@prefix dc: <http://purl.org/dc/elements/1.1/> .
@prefix rdf: <http://www.w3.org/1999/02/22-rdf-syntax-ns#> .
@prefix rdfs: <http://www.w3.org/2000/01/rdf-schema#> .
@prefix reg: <http://metadataregistry.org/uri/profile/regap/> .
@prefix skos: <http://www.w3.org/2004/02/skos/core#> .
@prefix xml: <http://www.w3.org/XML/1998/namespace> .
@prefix xsd: <http://www.w3.org/2001/XMLSchema#> .

<http://rdaregistry.info/termList/extentNoteMus/1001> a skos:Concept ;
    reg:identifier <http://metadataregistry.org/concepts/730> ;
    reg:status <http://metadataregistry.org/uri/RegStatus/1008> ;
    skos:altLabel "full score (Deprecated)"@en ;
    skos:definition "Graphical, symbolic, or word-based musical notation representing the sounds of all the parts of an ensemble or a work for solo performer or electronic media.  (Deprecated)"@en ;
    skos:inScheme <http://rdaregistry.info/termList/extenttNoteMus> ;
    skos:prefLabel "score (Deprecated)"@en ;
    skos:scopeNote "Do not confuse with Part."@en .

<http://rdaregistry.info/termList/extentNoteMus/1002> a skos:Concept ;
    reg:identifier <http://metadataregistry.org/concepts/731> ;
    reg:status <http://metadataregistry.org/uri/RegStatus/1008> ;
    skos:altLabel "reduced score (Deprecated)"@en,
        "short score"@en ;
    skos:definition "A score in which the number of staves is reduced to two or a few, generally organized by instrumental sections, and often with cues for individual parts.  (Deprecated)"@en ;
    skos:inScheme <http://rdaregistry.info/termList/extenttNoteMus> ;
    skos:prefLabel "condensed score (Deprecated)"@en .

<http://rdaregistry.info/termList/extentNoteMus/1003> a skos:Concept ;
    reg:identifier <http://metadataregistry.org/concepts/732> ;
    reg:status <http://metadataregistry.org/uri/RegStatus/1008> ;
    skos:definition "A score issued in a musical image of reduced size, not primarily intended for use in performance. A descriptive phrase such as \"Study score\", \"Miniature score\", \"Taschenpartitur\", \"Partition de poche\", etc., usually appears on the resource. (Deprecated)"@en ;
    skos:inScheme <http://rdaregistry.info/termList/extenttNoteMus> ;
    skos:prefLabel "study score (Deprecated)"@en .

<http://rdaregistry.info/termList/extentNoteMus/1004> a skos:Concept ;
    reg:identifier <http://metadataregistry.org/concepts/733> ;
    reg:status <http://metadataregistry.org/uri/RegStatus/1008> ;
    skos:definition "A performance part for a piano performer in an ensemble, with cues for the other instruments that enable the performer of that part also to conduct. (Deprecated)"@en ;
    skos:inScheme <http://rdaregistry.info/termList/extenttNoteMus> ;
    skos:prefLabel "piano conductor part (Deprecated)"@en .

<http://rdaregistry.info/termList/extentNoteMus/1005> a skos:Concept ;
    reg:identifier <http://metadataregistry.org/concepts/734> ;
    reg:status <http://metadataregistry.org/uri/RegStatus/1008> ;
    skos:definition "A performance part for a violin performer in an ensemble, with cues for the other instruments that enable the performer of that part also to conduct. (Deprecated)"@en ;
    skos:inScheme <http://rdaregistry.info/termList/extenttNoteMus> ;
    skos:prefLabel "violin conductor part (Deprecated)"@en .

<http://rdaregistry.info/termList/extentNoteMus/1006> a skos:Concept ;
    reg:identifier <http://metadataregistry.org/concepts/735> ;
    reg:status <http://metadataregistry.org/uri/RegStatus/1008> ;
    skos:definition "A score showing all vocal parts, with the instrumental accompaniment either arranged for keyboard(s) or other chordal instrument(s) or omitted. (Deprecated)"@en ;
    skos:inScheme <http://rdaregistry.info/termList/extenttNoteMus> ;
    skos:prefLabel "vocal score (Deprecated)"@en .

<http://rdaregistry.info/termList/extentNoteMus/1007> a skos:Concept ;
    reg:identifier <http://metadataregistry.org/concepts/736> ;
    reg:status <http://metadataregistry.org/uri/RegStatus/1008> ;
    skos:definition "A reduction of an instrumental work or a vocal work with instruments to a version for piano. May include the words of a vocal work. (Deprecated)"@en ;
    skos:inScheme <http://rdaregistry.info/termList/extenttNoteMus> ;
    skos:prefLabel "piano score (Deprecated)"@en .

<http://rdaregistry.info/termList/extentNoteMus/1008> a skos:Concept ;
    reg:identifier <http://metadataregistry.org/concepts/737> ;
    reg:status <http://metadataregistry.org/uri/RegStatus/1008> ;
    skos:definition "A score of a work for solo voices and chorus showing only the parts for chorus, at least in those portions of the work in which the chorus sings, with the instrumental accompaniment either arranged for keyboard(s) or other chordal instruments(s) or omitted. (Deprecated)"@en ;
    skos:inScheme <http://rdaregistry.info/termList/extenttNoteMus> ;
    skos:prefLabel "chorus score (Deprecated)"@en .

<http://rdaregistry.info/termList/extentNoteMus/1009> a skos:Concept ;
    reg:identifier <http://metadataregistry.org/concepts/738> ;
    reg:status <http://metadataregistry.org/uri/RegStatus/1008> ;
    skos:definition "In the context of notated music, a component consisting of the music for the use of one or more, but not all, performers. (Deprecated)"@en ;
    skos:inScheme <http://rdaregistry.info/termList/extenttNoteMus> ;
    skos:prefLabel "part (Deprecated)"@en .

<http://rdaregistry.info/termList/extentNoteMus/1010> a skos:Concept ;
    reg:identifier <http://metadataregistry.org/concepts/739> ;
    reg:status <http://metadataregistry.org/uri/RegStatus/1008> ;
    skos:definition "A large music book made to be placed on a stand in front of a choir. Each part is notated separately, usually in the configuration that presents, when the book is open, the soprano and tenor parts on the verso of a leaf, and the alto and bass parts on the recto of the next leaf. (Deprecated)"@en ;
    skos:inScheme <http://rdaregistry.info/termList/extenttNoteMus> ;
    skos:prefLabel "choir book (Deprecated)"@en .

<http://rdaregistry.info/termList/extentNoteMus/1011> a skos:Concept ;
    reg:identifier <http://metadataregistry.org/concepts/740> ;
    reg:status <http://metadataregistry.org/uri/RegStatus/1008> ;
    skos:definition "A music book made to be placed on a table and displayed in such a way that the performers can read their parts while seated or standing across or around the table. Each part is notated separately, usually in a configuration that presents, when the book is open, different parts in inverted and/or perpendicular positions. (Deprecated)"@en ;
    skos:inScheme <http://rdaregistry.info/termList/extenttNoteMus> ;
    skos:prefLabel "table book (Deprecated)"@en .

<http://rdaregistry.info/termList/extenttNoteMus/1013> a skos:Concept ;
    reg:identifier <http://metadataregistry.org/concepts/1093> ;
    reg:status <http://metadataregistry.org/uri/RegStatus/1008> ;
    skos:altLabel "full scores (Deprecated)"@en ;
    skos:definition "Graphical, symbolic, or word-based musical notation representing the sounds of all the parts of an ensemble or a work for solo performer or electronic media.  (Deprecated)"@en ;
    skos:inScheme <http://rdaregistry.info/termList/extenttNoteMus> ;
    skos:prefLabel "scores (Deprecated)"@en ;
    skos:scopeNote "Do not confuse with Parts."@en .

<http://rdaregistry.info/termList/extenttNoteMus/1014> a skos:Concept ;
    reg:identifier <http://metadataregistry.org/concepts/1094> ;
    reg:status <http://metadataregistry.org/uri/RegStatus/1008> ;
    skos:altLabel "reduced scores (Deprecated)"@en,
        "short scores"@en ;
    skos:definition "Scores in which the number of staves is reduced to two or a few, generally organized by instrumental sections, and often with cues for individual parts.  (Deprecated)"@en ;
    skos:inScheme <http://rdaregistry.info/termList/extenttNoteMus> ;
    skos:prefLabel "condensed scores (Deprecated)"@en .

<http://rdaregistry.info/termList/extenttNoteMus/1015> a skos:Concept ;
    reg:identifier <http://metadataregistry.org/concepts/1095> ;
    reg:status <http://metadataregistry.org/uri/RegStatus/1008> ;
    skos:definition "Scores issued in a musical image of reduced size, not primarily intended for use in performance. A descriptive phrase such as \"Study score\", \"Miniature score\", \"Taschenpartitur\", \"Partition de poche\", etc., usually appears on the resource. (Deprecated)"@en ;
    skos:inScheme <http://rdaregistry.info/termList/extenttNoteMus> ;
    skos:prefLabel "study scores (Deprecated)"@en .

<http://rdaregistry.info/termList/extenttNoteMus/1016> a skos:Concept ;
    reg:identifier <http://metadataregistry.org/concepts/1096> ;
    reg:status <http://metadataregistry.org/uri/RegStatus/1008> ;
    skos:definition "Performance parts for a piano performer in an ensemble, with cues for the other instruments that enable the performer of that part also to conduct. (Deprecated)"@en ;
    skos:inScheme <http://rdaregistry.info/termList/extenttNoteMus> ;
    skos:prefLabel "piano conductor parts (Deprecated)"@en .

<http://rdaregistry.info/termList/extenttNoteMus/1017> a skos:Concept ;
    reg:identifier <http://metadataregistry.org/concepts/1097> ;
    reg:status <http://metadataregistry.org/uri/RegStatus/1008> ;
    skos:definition "Performance parts for a violin performer in an ensemble, with cues for the other instruments that enable the performer of that part also to conduct. (Deprecated)"@en ;
    skos:inScheme <http://rdaregistry.info/termList/extenttNoteMus> ;
    skos:prefLabel "violin conductor parts (Deprecated)"@en .

<http://rdaregistry.info/termList/extenttNoteMus/1018> a skos:Concept ;
    reg:identifier <http://metadataregistry.org/concepts/1098> ;
    reg:status <http://metadataregistry.org/uri/RegStatus/1008> ;
    skos:definition "Scores showing all vocal parts, with the instrumental accompaniment either arranged for keyboard(s) or other chordal instrument(s) or omitted. (Deprecated)"@en ;
    skos:inScheme <http://rdaregistry.info/termList/extenttNoteMus> ;
    skos:prefLabel "vocal scores (Deprecated)"@en .

<http://rdaregistry.info/termList/extenttNoteMus/1019> a skos:Concept ;
    reg:identifier <http://metadataregistry.org/concepts/1099> ;
    reg:status <http://metadataregistry.org/uri/RegStatus/1008> ;
    skos:definition "Reductions of an instrumental work or a vocal work with instruments to a version for piano. May include the words of a vocal work. (Deprecated)"@en ;
    skos:inScheme <http://rdaregistry.info/termList/extenttNoteMus> ;
    skos:prefLabel "piano scores (Deprecated)"@en .

<http://rdaregistry.info/termList/extenttNoteMus/1020> a skos:Concept ;
    reg:identifier <http://metadataregistry.org/concepts/1100> ;
    reg:status <http://metadataregistry.org/uri/RegStatus/1008> ;
    skos:definition "Scores of a work for solo voices and chorus showing only the parts for chorus, at least in those portions of the work in which the chorus sings, with the instrumental accompaniment either arranged for keyboard(s) or other chordal instruments(s) or omitted. (Deprecated)"@en ;
    skos:inScheme <http://rdaregistry.info/termList/extenttNoteMus> ;
    skos:prefLabel "chorus scores (Deprecated)"@en .

<http://rdaregistry.info/termList/extenttNoteMus/1021> a skos:Concept ;
    reg:identifier <http://metadataregistry.org/concepts/1101> ;
    reg:status <http://metadataregistry.org/uri/RegStatus/1008> ;
    skos:definition "In the context of notated music, components consisting of the music for the use of one or more, but not all, performers. (Deprecated)"@en ;
    skos:inScheme <http://rdaregistry.info/termList/extenttNoteMus> ;
    skos:prefLabel "parts (Deprecated)"@en .

<http://rdaregistry.info/termList/extenttNoteMus/1022> a skos:Concept ;
    reg:identifier <http://metadataregistry.org/concepts/1102> ;
    reg:status <http://metadataregistry.org/uri/RegStatus/1008> ;
    skos:definition "Large music books made to be placed on a stand in front of a choir. Each part is notated separately, usually in the configuration that presents, when the book is open, the soprano and tenor parts on the verso of a leaf, and the alto and bass parts on the recto of the next leaf. (Deprecated)"@en ;
    skos:inScheme <http://rdaregistry.info/termList/extenttNoteMus> ;
    skos:prefLabel "choir books (Deprecated)"@en .

<http://rdaregistry.info/termList/extenttNoteMus/1023> a skos:Concept ;
    reg:identifier <http://metadataregistry.org/concepts/1103> ;
    reg:status <http://metadataregistry.org/uri/RegStatus/1008> ;
    skos:definition "Music books made to be placed on a table and displayed in such a way that the performers can read their parts while seated or standing across or around the table. Each part is notated separately, usually in a configuration that presents, when the book is open, different parts in inverted and/or perpendicular positions. (Deprecated)"@en ;
    skos:inScheme <http://rdaregistry.info/termList/extenttNoteMus> ;
    skos:prefLabel "table books (Deprecated)"@en .

<http://metadataregistry.org/uri/RegStatus/1008> a skos:Concept ;
    skos:prefLabel "Deprecated"@en .

<http://rdaregistry.info/termList/extenttNoteMus> a skos:ConceptScheme ;
    dc:title "RDA Extent of Notated Music (Deprecated)" .

