@prefix dc: <http://purl.org/dc/elements/1.1/> .
@prefix rdakit: <http://metadataregistry.org/uri/profile/rdakit/> .
@prefix rdf: <http://www.w3.org/1999/02/22-rdf-syntax-ns#> .
@prefix rdfs: <http://www.w3.org/2000/01/rdf-schema#> .
@prefix reg: <http://metadataregistry.org/uri/profile/regap/> .
@prefix skos: <http://www.w3.org/2004/02/skos/core#> .
@prefix xml: <http://www.w3.org/XML/1998/namespace> .
@prefix xsd: <http://www.w3.org/2001/XMLSchema#> .

<http://rdaregistry.info/termList/IllusContent/1001> a skos:Concept ;
    rdakit:toolkitDefinition "An illustrative content that includes the full display of armorial bearings consisting of the escutcheon plus its adjuncts."@en ;
    rdakit:toolkitLabel "coat of arms"@en ;
    reg:identifier <http://metadataregistry.org/concepts/714> ;
    reg:status <http://metadataregistry.org/uri/RegStatus/1001> ;
    skos:definition "An illustrative content that includes the full display of armorial bearings consisting of the escutcheon plus its adjuncts."@en ;
    skos:inScheme <http://rdaregistry.info/termList/IllusContent> ;
    skos:prefLabel "coat of arms"@en .

<http://rdaregistry.info/termList/IllusContent/1002> a skos:Concept ;
    rdakit:toolkitDefinition "An illustrative content consisting of an exact copy of an original, usually in the same dimensions as the original, especially of books, documents, prints, and drawings."@en ;
    rdakit:toolkitLabel "facsimile"@en ;
    reg:identifier <http://metadataregistry.org/concepts/715> ;
    reg:status <http://metadataregistry.org/uri/RegStatus/1001> ;
    skos:definition "An illustrative content consisting of an exact copy of an original, usually in the same dimensions as the original, especially of books, documents, prints, and drawings."@en ;
    skos:inScheme <http://rdaregistry.info/termList/IllusContent> ;
    skos:prefLabel "facsimile"@en ;
    skos:scopeNote "Today the original is often reproduced photographically or digitally; in the past, it was reproduced by engraving or other printmaking process."@en .

<http://rdaregistry.info/termList/IllusContent/1003> a skos:Concept ;
    rdakit:toolkitDefinition "An illustrative content consisting of labeled areas for recording structured data to be input by specified persons for specific purposes, usually accompanied by prompts and guidance."@en ;
    rdakit:toolkitLabel "form"@en ;
    reg:identifier <http://metadataregistry.org/concepts/716> ;
    reg:status <http://metadataregistry.org/uri/RegStatus/1001> ;
    skos:definition "An illustrative content consisting of labeled areas for recording structured data to be input by specified persons for specific purposes, usually accompanied by prompts and guidance."@en ;
    skos:inScheme <http://rdaregistry.info/termList/IllusContent> ;
    skos:prefLabel "form"@en .

<http://rdaregistry.info/termList/IllusContent/1004> a skos:Concept ;
    rdakit:toolkitDefinition "An illustrative content consisting of a table or diagram representing the lineage of a person or family."@en ;
    rdakit:toolkitLabel "genealogical table"@en ;
    reg:identifier <http://metadataregistry.org/concepts/717> ;
    reg:status <http://metadataregistry.org/uri/RegStatus/1001> ;
    skos:definition "An illustrative content consisting of a table or diagram representing the lineage of a person or family."@en ;
    skos:inScheme <http://rdaregistry.info/termList/IllusContent> ;
    skos:prefLabel "genealogical table"@en .

<http://rdaregistry.info/termList/IllusContent/1005> a skos:Concept ;
    rdakit:toolkitDefinition "An illustrative content consisting of a diagram showing relative quantitative and qualitative aspects of a data set."@en ;
    rdakit:toolkitLabel "graph"@en ;
    reg:identifier <http://metadataregistry.org/concepts/718> ;
    reg:status <http://metadataregistry.org/uri/RegStatus/1001> ;
    skos:definition "An illustrative content consisting of a diagram showing relative quantitative and qualitative aspects of a data set."@en ;
    skos:inScheme <http://rdaregistry.info/termList/IllusContent> ;
    skos:prefLabel "graph"@en .

<http://rdaregistry.info/termList/IllusContent/1006> a skos:Concept ;
    rdakit:toolkitDefinition "An illustrative content consisting of adornments, usually in one or more colours and applied by hand to an item using paint, ink, or metal foil."@en ;
    rdakit:toolkitLabel "illumination"@en ;
    reg:identifier <http://metadataregistry.org/concepts/719> ;
    reg:status <http://metadataregistry.org/uri/RegStatus/1001> ;
    skos:definition "An illustrative content consisting of adornments, usually in one or more colours and applied by hand to an item using paint, ink, or metal foil."@en ;
    skos:inScheme <http://rdaregistry.info/termList/IllusContent> ;
    skos:prefLabel "illumination"@en .

<http://rdaregistry.info/termList/IllusContent/1007> a skos:Concept ;
    reg:identifier <http://metadataregistry.org/concepts/720> ;
    reg:status <http://metadataregistry.org/uri/RegStatus/1008> ;
    skos:inScheme <http://rdaregistry.info/termList/IllusContent> ;
    skos:prefLabel "Illuminations (Deprecated)"@en .

<http://rdaregistry.info/termList/IllusContent/1008> a skos:Concept ;
    rdakit:toolkitDefinition "An illustrative content consisting of a representation, normally to scale and on a two-dimensional medium, of a selection of material or abstract features on, or in relation to, the surface of Earth, another celestial body, or an imaginary place."@en ;
    rdakit:toolkitLabel "map"@en ;
    reg:identifier <http://metadataregistry.org/concepts/721> ;
    reg:status <http://metadataregistry.org/uri/RegStatus/1001> ;
    skos:definition "An illustrative content consisting of a representation, normally to scale and on a two-dimensional medium, of a selection of material or abstract features on, or in relation to, the surface of Earth, another celestial body, or an imaginary place."@en ;
    skos:inScheme <http://rdaregistry.info/termList/IllusContent> ;
    skos:prefLabel "map"@en .

<http://rdaregistry.info/termList/IllusContent/1009> a skos:Concept ;
    rdakit:toolkitLabel "Music"@en ;
    reg:identifier <http://metadataregistry.org/concepts/722> ;
    reg:status <http://metadataregistry.org/uri/RegStatus/1008> ;
    skos:inScheme <http://rdaregistry.info/termList/IllusContent> ;
    skos:prefLabel "Music (Deprecated)"@en .

<http://rdaregistry.info/termList/IllusContent/1010> a skos:Concept ;
    rdakit:toolkitDefinition "An illustrative content consisting of an image created by light falling on a light-sensitive surface, usually photographic film or an electronic medium."@en ;
    rdakit:toolkitLabel "photograph"@en ;
    reg:identifier <http://metadataregistry.org/concepts/723> ;
    reg:status <http://metadataregistry.org/uri/RegStatus/1001> ;
    skos:definition "An illustrative content consisting of an image created by light falling on a light-sensitive surface, usually photographic film or an electronic medium."@en ;
    skos:inScheme <http://rdaregistry.info/termList/IllusContent> ;
    skos:prefLabel "photograph"@en .

<http://rdaregistry.info/termList/IllusContent/1011> a skos:Concept ;
    rdakit:toolkitDefinition "An illustrative content consisting of a detailed drawing or diagram."@en ;
    rdakit:toolkitLabel "plan"@en ;
    reg:identifier <http://metadataregistry.org/concepts/724> ;
    reg:status <http://metadataregistry.org/uri/RegStatus/1001> ;
    skos:definition "An illustrative content consisting of a detailed drawing or diagram."@en ;
    skos:inScheme <http://rdaregistry.info/termList/IllusContent> ;
    skos:prefLabel "plan"@en .

<http://rdaregistry.info/termList/IllusContent/1012> a skos:Concept ;
    rdakit:toolkitDefinition "An illustrative content consisting of a representation of an individual or group of persons or animals that is intended to capture a known or supposed likeness, especially the face of the individual."@en ;
    rdakit:toolkitLabel "portrait"@en ;
    reg:identifier <http://metadataregistry.org/concepts/725> ;
    reg:status <http://metadataregistry.org/uri/RegStatus/1001> ;
    skos:definition "An illustrative content consisting of a representation of an individual or group of persons or animals that is intended to capture a known or supposed likeness, especially the face of the individual."@en ;
    skos:inScheme <http://rdaregistry.info/termList/IllusContent> ;
    skos:prefLabel "portrait"@en .

<http://rdaregistry.info/termList/IllusContent/1013> a skos:Concept ;
    rdakit:toolkitDefinition "An illustrative content consisting of an individual unit, segment, or small quantity taken as evidence of the quality or character of the entire group or lot."@en ;
    rdakit:toolkitLabel "sample"@en ;
    reg:identifier <http://metadataregistry.org/concepts/726> ;
    reg:status <http://metadataregistry.org/uri/RegStatus/1001> ;
    skos:definition "An illustrative content consisting of an individual unit, segment, or small quantity taken as evidence of the quality or character of the entire group or lot."@en ;
    skos:inScheme <http://rdaregistry.info/termList/IllusContent> ;
    skos:prefLabel "sample"@en .

<http://rdaregistry.info/termList/IllusContent/1014> a skos:Concept ;
    rdakit:toolkitDefinition "An illustrative content consisting of a still image."@en ;
    rdakit:toolkitLabel "illustration"@en ;
    reg:identifier <http://metadataregistry.org/concepts/1024> ;
    reg:status <http://metadataregistry.org/uri/RegStatus/1001> ;
    skos:definition "An illustrative content consisting of a still image."@en ;
    skos:inScheme <http://rdaregistry.info/termList/IllusContent> ;
    skos:prefLabel "illustration"@en .

<http://rdaregistry.info/termList/IllusContent/1015> a skos:Concept ;
    reg:identifier <http://metadataregistry.org/concepts/1025> ;
    reg:status <http://metadataregistry.org/uri/RegStatus/1008> ;
    skos:inScheme <http://rdaregistry.info/termList/IllusContent> ;
    skos:prefLabel "Illustrations (Deprecated)"@en .

<http://metadataregistry.org/uri/RegStatus/1008> a skos:Concept ;
    skos:prefLabel "Deprecated"@en .

<http://metadataregistry.org/uri/RegStatus/1001> a skos:Concept ;
    skos:prefLabel "Published"@en .

<http://rdaregistry.info/termList/IllusContent> a skos:ConceptScheme ;
    dc:title "RDA Illustrative Content" .

