@prefix dc: <http://purl.org/dc/elements/1.1/> .
@prefix rdakit: <http://metadataregistry.org/uri/profile/rdakit/> .
@prefix rdf: <http://www.w3.org/1999/02/22-rdf-syntax-ns#> .
@prefix rdfs: <http://www.w3.org/2000/01/rdf-schema#> .
@prefix reg: <http://metadataregistry.org/uri/profile/regap/> .
@prefix skos: <http://www.w3.org/2004/02/skos/core#> .
@prefix xml: <http://www.w3.org/XML/1998/namespace> .
@prefix xsd: <http://www.w3.org/2001/XMLSchema#> .

<http://rdaregistry.info/termList/RDACarrierEU/1002> a skos:Concept ;
    rdakit:toolkitDefinition "A unit of extent that is a volume of maps or other cartographic content with or without descriptive text."@en ;
    rdakit:toolkitLabel "atlas"@en ;
    reg:identifier <http://metadataregistry.org/concepts/8624> ;
    reg:status <http://metadataregistry.org/uri/RegStatus/1001> ;
    skos:definition "A unit of extent that is a volume of maps or other cartographic content with or without descriptive text."@en ;
    skos:inScheme <http://rdaregistry.info/termList/RDACarrierEU> ;
    skos:prefLabel "atlas"@en ;
    skos:scopeNote "This term applies to cartographic resources."@en .

<http://rdaregistry.info/termList/RDACarrierEU/1003> a skos:Concept ;
    rdakit:toolkitDefinition "A unit of extent consisting of a box containing bound or unbound resources."@en ;
    rdakit:toolkitLabel "case"@en ;
    reg:identifier <http://metadataregistry.org/concepts/8625> ;
    reg:status <http://metadataregistry.org/uri/RegStatus/1001> ;
    skos:definition "A unit of extent consisting of a box containing bound or unbound resources."@en ;
    skos:inScheme <http://rdaregistry.info/termList/RDACarrierEU> ;
    skos:prefLabel "case"@en .

<http://rdaregistry.info/termList/RDACarrierEU/1004> a skos:Concept ;
    rdakit:toolkitDefinition "A unit of extent consisting of a two-dimensional representation of data in graphic or tabular form."@en ;
    rdakit:toolkitLabel "chart"@en ;
    reg:identifier <http://metadataregistry.org/concepts/8626> ;
    reg:status <http://metadataregistry.org/uri/RegStatus/1001> ;
    skos:definition "A unit of extent consisting of a two-dimensional representation of data in graphic or tabular form."@en ;
    skos:inScheme <http://rdaregistry.info/termList/RDACarrierEU> ;
    skos:prefLabel "chart"@en ;
    skos:scopeNote "This term applies to still images."@en .

<http://rdaregistry.info/termList/RDACarrierEU/1005> a skos:Concept ;
    rdakit:toolkitDefinition "A unit of extent consisting of a piece of metal stamped by government authority for use as money."@en ;
    rdakit:toolkitLabel "coin"@en ;
    reg:identifier <http://metadataregistry.org/concepts/8627> ;
    reg:status <http://metadataregistry.org/uri/RegStatus/1001> ;
    skos:definition "A unit of extent consisting of a piece of metal stamped by government authority for use as money."@en ;
    skos:inScheme <http://rdaregistry.info/termList/RDACarrierEU> ;
    skos:prefLabel "coin"@en ;
    skos:scopeNote "This term applies to three-dimensional forms."@en .

<http://rdaregistry.info/termList/RDACarrierEU/1006> a skos:Concept ;
    rdakit:toolkitDefinition "A unit of extent consisting of a work in two dimensions or very low relief that was made by affixing paper, fabrics, photographs, or other materials onto a flat surface."@en ;
    rdakit:toolkitLabel "collage"@en ;
    reg:identifier <http://metadataregistry.org/concepts/8628> ;
    reg:status <http://metadataregistry.org/uri/RegStatus/1001> ;
    skos:definition "A unit of extent consisting of a work in two dimensions or very low relief that was made by affixing paper, fabrics, photographs, or other materials onto a flat surface."@en ;
    skos:inScheme <http://rdaregistry.info/termList/RDACarrierEU> ;
    skos:prefLabel "collage"@en ;
    skos:scopeNote "This term applies to still images."@en .

<http://rdaregistry.info/termList/RDACarrierEU/1007> a skos:Concept ;
    rdakit:toolkitDefinition "A unit of extent consisting of one of two or more vertical sections of text appearing on the same page or leaf."@en ;
    rdakit:toolkitLabel "column"@en ;
    reg:identifier <http://metadataregistry.org/concepts/8629> ;
    reg:status <http://metadataregistry.org/uri/RegStatus/1001> ;
    skos:definition "A unit of extent consisting of one of two or more vertical sections of text appearing on the same page or leaf."@en ;
    skos:inScheme <http://rdaregistry.info/termList/RDACarrierEU> ;
    skos:prefLabel "column"@en .

<http://rdaregistry.info/termList/RDACarrierEU/1008> a skos:Concept ;
    rdakit:toolkitDefinition "A unit of extent that is a geographic representation of numeric data, or of the course or results of an action or process."@en ;
    rdakit:toolkitLabel "diagram"@en ;
    reg:identifier <http://metadataregistry.org/concepts/8630> ;
    reg:status <http://metadataregistry.org/uri/RegStatus/1001> ;
    skos:definition "A unit of extent that is a geographic representation of numeric data, or of the course or results of an action or process."@en ;
    skos:inScheme <http://rdaregistry.info/termList/RDACarrierEU> ;
    skos:prefLabel "diagram"@en ;
    skos:scopeNote "This term applies to cartographic resources. The term is sometimes also applied to maps characterized by much simplified, or schematic, representation."@en .

<http://rdaregistry.info/termList/RDACarrierEU/1009> a skos:Concept ;
    rdakit:toolkitDefinition "A unit of extent consisting of a three-dimensional representation of a scene created by placing objects, figures, etc., in front of a two-dimensional painted background."@en ;
    rdakit:toolkitLabel "diorama"@en ;
    reg:identifier <http://metadataregistry.org/concepts/8631> ;
    reg:status <http://metadataregistry.org/uri/RegStatus/1001> ;
    skos:definition "A unit of extent consisting of a three-dimensional representation of a scene created by placing objects, figures, etc., in front of a two-dimensional painted background."@en ;
    skos:inScheme <http://rdaregistry.info/termList/RDACarrierEU> ;
    skos:prefLabel "diorama"@en ;
    skos:scopeNote "This term applies to three-dimensional forms."@en .

<http://rdaregistry.info/termList/RDACarrierEU/1010> a skos:Concept ;
    rdakit:toolkitDefinition "A unit of extent consisting of a visual work produced by drawing, which is the application of lines on a surface, often paper, by using a pencil, pen, chalk, or some other tracing instrument to focus on the delineation of form rather than the application of color."@en ;
    rdakit:toolkitLabel "drawing"@en ;
    reg:identifier <http://metadataregistry.org/concepts/8632> ;
    reg:status <http://metadataregistry.org/uri/RegStatus/1001> ;
    skos:definition "A unit of extent consisting of a visual work produced by drawing, which is the application of lines on a surface, often paper, by using a pencil, pen, chalk, or some other tracing instrument to focus on the delineation of form rather than the application of color."@en ;
    skos:inScheme <http://rdaregistry.info/termList/RDACarrierEU> ;
    skos:prefLabel "drawing"@en ;
    skos:scopeNote "This term applies to still images. This term is often defined broadly to refer to computer-generated images as well."@en .

<http://rdaregistry.info/termList/RDACarrierEU/1011> a skos:Concept ;
    rdakit:toolkitDefinition "A unit of extent consisting of objects on display, along with the display environment of cases, labels, etc."@en ;
    rdakit:toolkitLabel "exhibit"@en ;
    reg:identifier <http://metadataregistry.org/concepts/8633> ;
    reg:status <http://metadataregistry.org/uri/RegStatus/1001> ;
    skos:definition "A unit of extent consisting of objects on display, along with the display environment of cases, labels, etc."@en ;
    skos:inScheme <http://rdaregistry.info/termList/RDACarrierEU> ;
    skos:prefLabel "exhibit"@en ;
    skos:scopeNote "This term applies to three-dimensional forms."@en .

<http://rdaregistry.info/termList/RDACarrierEU/1012> a skos:Concept ;
    rdakit:toolkitDefinition "A unit of extent consisting of a card, or digital representation of a card, carrying words, numerals, pictures, etc., designed for rapid display as an aid to learning."@en ;
    rdakit:toolkitLabel "flash card"@en ;
    reg:identifier <http://metadataregistry.org/concepts/8634> ;
    reg:status <http://metadataregistry.org/uri/RegStatus/1001> ;
    skos:altLabel "electronic flash card"@en ;
    skos:definition "A unit of extent consisting of a card, or digital representation of a card, carrying words, numerals, pictures, etc., designed for rapid display as an aid to learning."@en ;
    skos:inScheme <http://rdaregistry.info/termList/RDACarrierEU> ;
    skos:prefLabel "flash card"@en ;
    skos:scopeNote "This term applies to still images."@en .

<http://rdaregistry.info/termList/RDACarrierEU/1013> a skos:Concept ;
    rdakit:toolkitDefinition "A unit of extent consisting of a sheet designed to be read in pages when folded."@en ;
    rdakit:toolkitLabel "folded sheet"@en ;
    reg:identifier <http://metadataregistry.org/concepts/8635> ;
    reg:status <http://metadataregistry.org/uri/RegStatus/1001> ;
    skos:definition "A unit of extent consisting of a sheet designed to be read in pages when folded."@en ;
    skos:inScheme <http://rdaregistry.info/termList/RDACarrierEU> ;
    skos:prefLabel "folded sheet"@en .

<http://rdaregistry.info/termList/RDACarrierEU/1015> a skos:Concept ;
    rdakit:toolkitDefinition "A unit of extent that is a depiction of the Earth or other celestial body, real or imaginary, on the surface of a sphere."@en ;
    rdakit:toolkitLabel "globe"@en ;
    reg:identifier <http://metadataregistry.org/concepts/8637> ;
    reg:status <http://metadataregistry.org/uri/RegStatus/1001> ;
    skos:definition "A unit of extent that is a depiction of the Earth or other celestial body, real or imaginary, on the surface of a sphere."@en ;
    skos:inScheme <http://rdaregistry.info/termList/RDACarrierEU> ;
    skos:prefLabel "globe"@en ;
    skos:scopeNote "This term applies to cartographic resources."@en .

<http://rdaregistry.info/termList/RDACarrierEU/1016> a skos:Concept ;
    rdakit:toolkitDefinition "A unit of extent consisting of an image that portrays a sacred entity and that is itself regarded as sacred."@en ;
    rdakit:toolkitLabel "icon"@en ;
    reg:identifier <http://metadataregistry.org/concepts/8638> ;
    reg:status <http://metadataregistry.org/uri/RegStatus/1001> ;
    skos:definition "A unit of extent consisting of an image that portrays a sacred entity and that is itself regarded as sacred."@en ;
    skos:inScheme <http://rdaregistry.info/termList/RDACarrierEU> ;
    skos:prefLabel "icon"@en ;
    skos:scopeNote "This term applies to still images. Most commonly it comprises tempera on panel, but it may be in any two-dimensional or relief medium, including fresco."@en .

<http://rdaregistry.info/termList/RDACarrierEU/1017> a skos:Concept ;
    rdakit:toolkitDefinition "A unit of extent consisting of a picture usually on pasteboard or wood, which has been cut into interlocking shapes intended to be re-assembled."@en ;
    rdakit:toolkitLabel "jigsaw puzzle"@en ;
    reg:identifier <http://metadataregistry.org/concepts/8639> ;
    reg:status <http://metadataregistry.org/uri/RegStatus/1001> ;
    skos:definition "A unit of extent consisting of a picture usually on pasteboard or wood, which has been cut into interlocking shapes intended to be re-assembled."@en ;
    skos:inScheme <http://rdaregistry.info/termList/RDACarrierEU> ;
    skos:prefLabel "jigsaw puzzle"@en ;
    skos:scopeNote "This term applies to three-dimensional forms."@en .

<http://rdaregistry.info/termList/RDACarrierEU/1018> a skos:Concept ;
    rdakit:toolkitDefinition "A unit of extent consisting of a single bound or fastened sheet as a subunit of a volume; each leaf consists of two pages, one on each side, either or both of which may be blank."@en ;
    rdakit:toolkitLabel "leaf"@en ;
    reg:identifier <http://metadataregistry.org/concepts/8640> ;
    reg:status <http://metadataregistry.org/uri/RegStatus/1001> ;
    skos:definition "A unit of extent consisting of a single bound or fastened sheet as a subunit of a volume; each leaf consists of two pages, one on each side, either or both of which may be blank."@en ;
    skos:inScheme <http://rdaregistry.info/termList/RDACarrierEU> ;
    skos:prefLabel "leaf"@en .

<http://rdaregistry.info/termList/RDACarrierEU/1019> a skos:Concept ;
    rdakit:toolkitDefinition "A unit of extent consisting of a representation, normally to scale and on a two-dimensional medium, of a selection of material or abstract features on, or in relation to, the surface of Earth, another celestial body, or an imaginary place."@en ;
    rdakit:toolkitLabel "map"@en ;
    reg:identifier <http://metadataregistry.org/concepts/8641> ;
    reg:status <http://metadataregistry.org/uri/RegStatus/1001> ;
    skos:definition "A unit of extent consisting of a representation, normally to scale and on a two-dimensional medium, of a selection of material or abstract features on, or in relation to, the surface of Earth, another celestial body, or an imaginary place."@en ;
    skos:inScheme <http://rdaregistry.info/termList/RDACarrierEU> ;
    skos:prefLabel "map"@en ;
    skos:scopeNote "This term applies to cartographic resources."@en .

<http://rdaregistry.info/termList/RDACarrierEU/1020> a skos:Concept ;
    rdakit:toolkitDefinition "A unit of extent consisting of a small piece of metal, bearing a relief design on one or both sides and having a commemorative purpose; not used as a medium of exchange."@en ;
    rdakit:toolkitLabel "medal"@en ;
    reg:identifier <http://metadataregistry.org/concepts/8642> ;
    reg:status <http://metadataregistry.org/uri/RegStatus/1001> ;
    skos:definition "A unit of extent consisting of a small piece of metal, bearing a relief design on one or both sides and having a commemorative purpose; not used as a medium of exchange."@en ;
    skos:inScheme <http://rdaregistry.info/termList/RDACarrierEU> ;
    skos:prefLabel "medal"@en ;
    skos:scopeNote "This term applies to three-dimensional forms."@en .

<http://rdaregistry.info/termList/RDACarrierEU/1021> a skos:Concept ;
    rdakit:toolkitDefinition "A unit of extent consisting of a physical representation of a device or process that may be modified for training or analysis to emphasize a particular part or function."@en ;
    rdakit:toolkitLabel "mock-up"@en ;
    reg:identifier <http://metadataregistry.org/concepts/8643> ;
    reg:status <http://metadataregistry.org/uri/RegStatus/1001> ;
    skos:definition "A unit of extent consisting of a physical representation of a device or process that may be modified for training or analysis to emphasize a particular part or function."@en ;
    skos:inScheme <http://rdaregistry.info/termList/RDACarrierEU> ;
    skos:prefLabel "mock-up"@en ;
    skos:scopeNote "This term applies to three-dimensional forms."@en .

<http://rdaregistry.info/termList/RDACarrierEU/1023> a skos:Concept ;
    rdakit:toolkitDefinition "A unit of extent consisting of a single side of a leaf."@en ;
    rdakit:toolkitLabel "page"@en ;
    reg:identifier <http://metadataregistry.org/concepts/8645> ;
    reg:status <http://metadataregistry.org/uri/RegStatus/1001> ;
    skos:definition "A unit of extent consisting of a single side of a leaf."@en ;
    skos:inScheme <http://rdaregistry.info/termList/RDACarrierEU> ;
    skos:prefLabel "page"@en .

<http://rdaregistry.info/termList/RDACarrierEU/1024> a skos:Concept ;
    rdakit:toolkitDefinition "A unit of extent consisting of an item in which images are formed primarily by the direct application of pigment suspended in a medium, arranged in masses of colour onto a generally two-dimensional surface."@en ;
    rdakit:toolkitLabel "painting"@en ;
    reg:identifier <http://metadataregistry.org/concepts/8646> ;
    reg:status <http://metadataregistry.org/uri/RegStatus/1001> ;
    skos:definition "A unit of extent consisting of an item in which images are formed primarily by the direct application of pigment suspended in a medium, arranged in masses of colour onto a generally two-dimensional surface."@en ;
    skos:inScheme <http://rdaregistry.info/termList/RDACarrierEU> ;
    skos:prefLabel "painting"@en ;
    skos:scopeNote "This term applies to still images."@en .

<http://rdaregistry.info/termList/RDACarrierEU/1025> a skos:Concept ;
    rdakit:toolkitDefinition "A unit of extent consisting of an image captured by a lens and carried on the surface of a sheet."@en ;
    rdakit:toolkitLabel "photograph"@en ;
    reg:identifier <http://metadataregistry.org/concepts/8647> ;
    reg:status <http://metadataregistry.org/uri/RegStatus/1001> ;
    skos:definition "A unit of extent consisting of an image captured by a lens and carried on the surface of a sheet."@en ;
    skos:inScheme <http://rdaregistry.info/termList/RDACarrierEU> ;
    skos:prefLabel "photograph"@en .

<http://rdaregistry.info/termList/RDACarrierEU/1026> a skos:Concept ;
    rdakit:toolkitDefinition "A unit of extent consisting of two-dimensional representations."@en ;
    rdakit:toolkitLabel "picture"@en ;
    reg:identifier <http://metadataregistry.org/concepts/8648> ;
    reg:status <http://metadataregistry.org/uri/RegStatus/1001> ;
    skos:definition "A unit of extent consisting of two-dimensional representations."@en ;
    skos:inScheme <http://rdaregistry.info/termList/RDACarrierEU> ;
    skos:prefLabel "picture"@en ;
    skos:scopeNote "This term applies to still images."@en .

<http://rdaregistry.info/termList/RDACarrierEU/1027> a skos:Concept ;
    rdakit:toolkitDefinition "A unit of extent that is a container for holding loose materials, usually consisting of two covers joined together at the back."@en ;
    rdakit:toolkitLabel "portfolio"@en ;
    reg:identifier <http://metadataregistry.org/concepts/8649> ;
    reg:status <http://metadataregistry.org/uri/RegStatus/1001> ;
    skos:definition "A unit of extent that is a container for holding loose materials, usually consisting of two covers joined together at the back."@en ;
    skos:inScheme <http://rdaregistry.info/termList/RDACarrierEU> ;
    skos:prefLabel "portfolio"@en .

<http://rdaregistry.info/termList/RDACarrierEU/1028> a skos:Concept ;
    rdakit:toolkitDefinition "A unit of extent of consisting of a card on which a message may be written or printed for mailing without an envelope."@en ;
    rdakit:toolkitLabel "postcard"@en ;
    reg:identifier <http://metadataregistry.org/concepts/8650> ;
    reg:status <http://metadataregistry.org/uri/RegStatus/1001> ;
    skos:definition "A unit of extent of consisting of a card on which a message may be written or printed for mailing without an envelope."@en ;
    skos:inScheme <http://rdaregistry.info/termList/RDACarrierEU> ;
    skos:prefLabel "postcard"@en ;
    skos:scopeNote "This term applies to still images."@en .

<http://rdaregistry.info/termList/RDACarrierEU/1029> a skos:Concept ;
    rdakit:toolkitDefinition "A unit of extent consisting of a notice, usually decorative or pictorial, intended to be posted to advertise, promote, or publicize an activity, cause, product, or service; also, a decorative, mass-produced print intended for hanging."@en ;
    rdakit:toolkitLabel "poster"@en ;
    reg:identifier <http://metadataregistry.org/concepts/8651> ;
    reg:status <http://metadataregistry.org/uri/RegStatus/1001> ;
    skos:definition "A unit of extent consisting of a notice, usually decorative or pictorial, intended to be posted to advertise, promote, or publicize an activity, cause, product, or service; also, a decorative, mass-produced print intended for hanging."@en ;
    skos:inScheme <http://rdaregistry.info/termList/RDACarrierEU> ;
    skos:prefLabel "poster"@en ;
    skos:scopeNote "This term applies to still images."@en .

<http://rdaregistry.info/termList/RDACarrierEU/1030> a skos:Concept ;
    rdakit:toolkitDefinition "A unit of extent consisting of a pictorial work produced by transferring an image by means of a matrix such as a plate, block, or screen, using any of various printing processes."@en ;
    rdakit:toolkitLabel "print"@en ;
    reg:identifier <http://metadataregistry.org/concepts/8652> ;
    reg:status <http://metadataregistry.org/uri/RegStatus/1001> ;
    skos:definition "A unit of extent consisting of a pictorial work produced by transferring an image by means of a matrix such as a plate, block, or screen, using any of various printing processes."@en ;
    skos:inScheme <http://rdaregistry.info/termList/RDACarrierEU> ;
    skos:prefLabel "print"@en ;
    skos:scopeNote "This term applies to still images."@en .

<http://rdaregistry.info/termList/RDACarrierEU/1031> a skos:Concept ;
    rdakit:toolkitDefinition "A unit of extent that is a scale representation of the intersection of a vertical surface, which may or may not be a plane, with the surface of the ground, or of the intersection of such a vertical surface with that of a conceptual three-dimensional model representing phenomena having a continuous distribution."@en ;
    rdakit:toolkitLabel "profile"@en ;
    reg:identifier <http://metadataregistry.org/concepts/8653> ;
    reg:status <http://metadataregistry.org/uri/RegStatus/1001> ;
    skos:definition "A unit of extent that is a scale representation of the intersection of a vertical surface, which may or may not be a plane, with the surface of the ground, or of the intersection of such a vertical surface with that of a conceptual three-dimensional model representing phenomena having a continuous distribution."@en ;
    skos:inScheme <http://rdaregistry.info/termList/RDACarrierEU> ;
    skos:prefLabel "profile"@en ;
    skos:scopeNote "This term applies to cartographic resources."@en .

<http://rdaregistry.info/termList/RDACarrierEU/1032> a skos:Concept ;
    rdakit:toolkitDefinition "A unit of extent that is a photograph produced by the passage of radiation, such as X rays, gamma rays, or neutrons, through an opaque object."@en ;
    rdakit:toolkitLabel "radiograph"@en ;
    reg:identifier <http://metadataregistry.org/concepts/8654> ;
    reg:status <http://metadataregistry.org/uri/RegStatus/1001> ;
    skos:definition "A unit of extent that is a photograph produced by the passage of radiation, such as X rays, gamma rays, or neutrons, through an opaque object."@en ;
    skos:inScheme <http://rdaregistry.info/termList/RDACarrierEU> ;
    skos:prefLabel "radiograph"@en .

<http://rdaregistry.info/termList/RDACarrierEU/1033> a skos:Concept ;
    rdakit:toolkitDefinition "A unit of extent that is a pictorial product of any remote-sensing instrument that detects and measures reflected and/or emitted electromagnetic radiation from a distance and reflected underwater sound waves in the case of sonar."@en ;
    rdakit:toolkitLabel "remote-sensing image"@en ;
    reg:identifier <http://metadataregistry.org/concepts/8655> ;
    reg:status <http://metadataregistry.org/uri/RegStatus/1001> ;
    skos:definition "A unit of extent that is a pictorial product of any remote-sensing instrument that detects and measures reflected and/or emitted electromagnetic radiation from a distance and reflected underwater sound waves in the case of sonar."@en ;
    skos:inScheme <http://rdaregistry.info/termList/RDACarrierEU> ;
    skos:prefLabel "remote-sensing image"@en ;
    skos:scopeNote "This term applies to cartographic resources."@en .

<http://rdaregistry.info/termList/RDACarrierEU/1034> a skos:Concept ;
    rdakit:toolkitDefinition "A unit of extent consisting of a physical representation, usually of art, in which an image or form is produced in relief, in intaglio, or in the round."@en ;
    rdakit:toolkitLabel "sculpture"@en ;
    reg:identifier <http://metadataregistry.org/concepts/8656> ;
    reg:status <http://metadataregistry.org/uri/RegStatus/1001> ;
    skos:definition "A unit of extent consisting of a physical representation, usually of art, in which an image or form is produced in relief, in intaglio, or in the round."@en ;
    skos:inScheme <http://rdaregistry.info/termList/RDACarrierEU> ;
    skos:prefLabel "sculpture"@en ;
    skos:scopeNote "This term applies to three-dimensional forms."@en .

<http://rdaregistry.info/termList/RDACarrierEU/1035> a skos:Concept ;
    rdakit:toolkitDefinition "A unit of extent that is a scale representation of a vertical surface, commonly a plane, displaying both the profile where it intersects the surface of a celestial body, or some conceptual model, and the underlying structures along the plane of intersection."@en ;
    rdakit:toolkitLabel "section"@en ;
    reg:identifier <http://metadataregistry.org/concepts/8657> ;
    reg:status <http://metadataregistry.org/uri/RegStatus/1001> ;
    skos:altLabel "map section"@en ;
    skos:definition "A unit of extent that is a scale representation of a vertical surface, commonly a plane, displaying both the profile where it intersects the surface of a celestial body, or some conceptual model, and the underlying structures along the plane of intersection."@en ;
    skos:inScheme <http://rdaregistry.info/termList/RDACarrierEU> ;
    skos:prefLabel "section"@en ;
    skos:scopeNote "This term applies to cartographic resources."@en .

<http://rdaregistry.info/termList/RDACarrierEU/1036> a skos:Concept ;
    rdakit:toolkitDefinition "A unit of extent consisting of an individual unit or sample chosen to represent a larger population or aggregation."@en ;
    rdakit:toolkitLabel "specimen"@en ;
    reg:identifier <http://metadataregistry.org/concepts/8658> ;
    reg:status <http://metadataregistry.org/uri/RegStatus/1001> ;
    skos:definition "A unit of extent consisting of an individual unit or sample chosen to represent a larger population or aggregation."@en ;
    skos:inScheme <http://rdaregistry.info/termList/RDACarrierEU> ;
    skos:prefLabel "specimen"@en ;
    skos:scopeNote "This term applies to three-dimensional forms."@en .

<http://rdaregistry.info/termList/RDACarrierEU/1037> a skos:Concept ;
    rdakit:toolkitDefinition "A unit of extent consisting of an image sometimes accompanied by text and used for education."@en ;
    rdakit:toolkitLabel "study print"@en ;
    reg:identifier <http://metadataregistry.org/concepts/8659> ;
    reg:status <http://metadataregistry.org/uri/RegStatus/1001> ;
    skos:definition "A unit of extent consisting of an image sometimes accompanied by text and used for education."@en ;
    skos:inScheme <http://rdaregistry.info/termList/RDACarrierEU> ;
    skos:prefLabel "study print"@en .

<http://rdaregistry.info/termList/RDACarrierEU/1038> a skos:Concept ;
    rdakit:toolkitDefinition "A unit of extent consisting of a cross section, detail, diagram, elevation, perspective, plan, working plan, etc., made for use in an engineering or other technical context."@en ;
    rdakit:toolkitLabel "technical drawing"@en ;
    reg:identifier <http://metadataregistry.org/concepts/8660> ;
    reg:status <http://metadataregistry.org/uri/RegStatus/1001> ;
    skos:definition "A unit of extent consisting of a cross section, detail, diagram, elevation, perspective, plan, working plan, etc., made for use in an engineering or other technical context."@en ;
    skos:inScheme <http://rdaregistry.info/termList/RDACarrierEU> ;
    skos:prefLabel "technical drawing"@en ;
    skos:scopeNote "This term applies to still images."@en .

<http://rdaregistry.info/termList/RDACarrierEU/1040> a skos:Concept ;
    rdakit:toolkitDefinition "A unit of extent that is a perspective representation of the landscape in which detail is shown as if projected on an oblique plane."@en ;
    rdakit:toolkitLabel "view"@en ;
    reg:identifier <http://metadataregistry.org/concepts/8662> ;
    reg:status <http://metadataregistry.org/uri/RegStatus/1001> ;
    skos:definition "A unit of extent that is a perspective representation of the landscape in which detail is shown as if projected on an oblique plane."@en ;
    skos:inScheme <http://rdaregistry.info/termList/RDACarrierEU> ;
    skos:prefLabel "view"@en ;
    skos:scopeNote "This term applies to cartographic resources. A bird’s-eye view, panorama, panoramic drawing, worm’s-eye view, etc., are included."@en .

<http://rdaregistry.info/termList/RDACarrierEU/1041> a skos:Concept ;
    rdakit:toolkitDefinition "A unit of extent consisting of a tabular or graphic representation of data appropriate for display on a wall."@en ;
    rdakit:toolkitLabel "wall chart"@en ;
    reg:identifier <http://metadataregistry.org/concepts/8663> ;
    reg:status <http://metadataregistry.org/uri/RegStatus/1001> ;
    skos:definition "A unit of extent consisting of a tabular or graphic representation of data appropriate for display on a wall."@en ;
    skos:inScheme <http://rdaregistry.info/termList/RDACarrierEU> ;
    skos:prefLabel "wall chart"@en ;
    skos:scopeNote "This term applies to still images."@en .

<http://rdaregistry.info/termList/RDACarrierEU/1001> a skos:Concept ;
    rdakit:toolkitDefinition "A unit of extent that is a card printed with words, numerals, and/or pictures to be used by an individual or a group as a basis for performing a specific activity."@en ;
    rdakit:toolkitLabel "activity card"@en ;
    reg:identifier <http://metadataregistry.org/concepts/8623> ;
    reg:status <http://metadataregistry.org/uri/RegStatus/1001> ;
    skos:definition "A unit of extent that is a card printed with words, numerals, and/or pictures to be used by an individual or a group as a basis for performing a specific activity."@en ;
    skos:inScheme <http://rdaregistry.info/termList/RDACarrierEU> ;
    skos:prefLabel "activity card"@en ;
    skos:related <http://rdaregistry.info/termList/RDACarrierEU/1039> ;
    skos:scopeNote "This term applies to still images. The cards are usually issued in sets."@en .

<http://rdaregistry.info/termList/RDACarrierEU/1014> a skos:Concept ;
    rdakit:toolkitDefinition "A unit of extent consisting of a set of objects designed for manipulation according to prescribed or implicit rules for education, entertainment, or therapy."@en ;
    rdakit:toolkitLabel "game"@en ;
    reg:identifier <http://metadataregistry.org/concepts/8636> ;
    reg:status <http://metadataregistry.org/uri/RegStatus/1001> ;
    skos:definition "A unit of extent consisting of a set of objects designed for manipulation according to prescribed or implicit rules for education, entertainment, or therapy."@en ;
    skos:inScheme <http://rdaregistry.info/termList/RDACarrierEU> ;
    skos:prefLabel "game"@en ;
    skos:related <http://rdaregistry.info/termList/RDACarrierEU/1039> ;
    skos:scopeNote "This term applies to three-dimensional forms."@en .

<http://rdaregistry.info/termList/RDACarrierEU/1022> a skos:Concept ;
    rdakit:toolkitDefinition "A unit of extent consisting of a three-dimensional representation of a real or imagined object."@en ;
    rdakit:toolkitLabel "model"@en ;
    reg:identifier <http://metadataregistry.org/concepts/8644> ;
    reg:status <http://metadataregistry.org/uri/RegStatus/1001> ;
    skos:definition "A unit of extent consisting of a three-dimensional representation of a real or imagined object."@en ;
    skos:inScheme <http://rdaregistry.info/termList/RDACarrierEU> ;
    skos:prefLabel "model"@en ;
    skos:related <http://rdaregistry.info/termList/RDACarrierEU/1039> ;
    skos:scopeNote "This term applies to cartographic resources and three-dimensional forms."@en .

<http://rdaregistry.info/termList/RDACarrierEU/1039> a skos:Concept ;
    rdakit:toolkitDefinition "A unit of extent consisting of an object designed for education, entertainment, or stimulation through play."@en ;
    rdakit:toolkitLabel "toy"@en ;
    reg:identifier <http://metadataregistry.org/concepts/8661> ;
    reg:status <http://metadataregistry.org/uri/RegStatus/1001> ;
    skos:definition "A unit of extent consisting of an object designed for education, entertainment, or stimulation through play."@en ;
    skos:inScheme <http://rdaregistry.info/termList/RDACarrierEU> ;
    skos:prefLabel "toy"@en ;
    skos:related <http://rdaregistry.info/termList/RDACarrierEU/1001>,
        <http://rdaregistry.info/termList/RDACarrierEU/1014>,
        <http://rdaregistry.info/termList/RDACarrierEU/1022> ;
    skos:scopeNote "This term applies to three-dimensional forms."@en .

<http://metadataregistry.org/uri/RegStatus/1001> a skos:Concept ;
    skos:prefLabel "Published"@en .

<http://rdaregistry.info/termList/RDACarrierEU> a skos:ConceptScheme ;
    dc:title "RDA Carrier Extent Unit" .

