@prefix dc: <http://purl.org/dc/elements/1.1/> .
@prefix rdakit: <http://metadataregistry.org/uri/profile/rdakit/> .
@prefix rdf: <http://www.w3.org/1999/02/22-rdf-syntax-ns#> .
@prefix rdfs: <http://www.w3.org/2000/01/rdf-schema#> .
@prefix reg: <http://metadataregistry.org/uri/profile/regap/> .
@prefix skos: <http://www.w3.org/2004/02/skos/core#> .
@prefix xml: <http://www.w3.org/XML/1998/namespace> .
@prefix xsd: <http://www.w3.org/2001/XMLSchema#> .

<http://rdaregistry.info/termList/RDAMaterial/1002> a skos:Concept ;
    rdakit:toolkitDefinition "A material consisting of pigment or dye bound in an emulsion of acrylic resin."@en ;
    rdakit:toolkitLabel "acrylic paint"@en ;
    reg:identifier <http://metadataregistry.org/concepts/8456> ;
    reg:status <http://metadataregistry.org/uri/RegStatus/1001> ;
    skos:definition "A material consisting of pigment or dye bound in an emulsion of acrylic resin."@en ;
    skos:inScheme <http://rdaregistry.info/termList/RDAMaterial> ;
    skos:prefLabel "acrylic paint"@en .

<http://rdaregistry.info/termList/RDAMaterial/1003> a skos:Concept ;
    rdakit:toolkitDefinition "A material of non-magnetic metal, usually alloyed, that is ductile and malleable with a lustre that ranges from grey to silver."@en,
        "Een basismateriaal van niet-magnetisch metaal, meestal gelegeerd, dat taai en kneedbaar is met een glans die varieert van grijs naar zilver."@nl,
        "具有延展性和可塑性、通常为合金、色泽在灰色至银色范围间的非磁性金属基底材料。"@zh ;
    rdakit:toolkitLabel "aluminium"@en,
        "aluminium"@nl,
        "aluminium"@sv,
        "铝"@zh ;
    reg:identifier <http://metadataregistry.org/concepts/8457> ;
    reg:status <http://metadataregistry.org/uri/RegStatus/1001> ;
    skos:altLabel "aluminum"@en ;
    skos:definition "A material of non-magnetic metal, usually alloyed, that is ductile and malleable with a lustre that ranges from grey to silver."@en,
        "Een basismateriaal van niet-magnetisch metaal, meestal gelegeerd, dat taai en kneedbaar is met een glans die varieert van grijs naar zilver."@nl,
        "具有延展性和可塑性、通常为合金、色泽在灰色至银色范围间的非磁性金属基底材料。"@zh ;
    skos:inScheme <http://rdaregistry.info/termList/RDAMaterial> ;
    skos:prefLabel "aluminium"@en,
        "aluminium"@nl,
        "aluminium"@sv,
        "铝"@zh .

<http://rdaregistry.info/termList/RDAMaterial/1004> a skos:Concept ;
    rdakit:toolkitDefinition "Ein Trägermaterial, das aus hochweißem Karton besteht, der mit Porzellanerde superkalandriert wurde oder durch Zusammenkleben von Blättern aus schwerem Ledger-Papier gemacht wird."@de,
        "A material consisting of a high-grade white cardboard, most commonly made by pasting together sheets of heavy ledger paper."@en,
        "Een basismateriaal bestaande uit een hoogwaardig wit karton, meestal gemaakt door vellen zwaar registerpapier aan elkaar te plakken."@nl,
        "由陶土经超级压光或厚帐薄纸粘贴而成的上等白色纸板构成的基底材料。"@zh ;
    rdakit:toolkitLabel "Bristolkarton"@de,
        "Bristol board"@en,
        "cartulina brístol"@es,
        "bristol"@fr,
        "bristolkarton"@nl,
        "Bristol board"@sv,
        "上等纸板/布里斯托纸板"@zh ;
    reg:identifier <http://metadataregistry.org/concepts/8458> ;
    reg:status <http://metadataregistry.org/uri/RegStatus/1001> ;
    skos:definition "Ein Trägermaterial, das aus hochweißem Karton besteht, der mit Porzellanerde superkalandriert wurde oder durch Zusammenkleben von Blättern aus schwerem Ledger-Papier gemacht wird."@de,
        "A material consisting of a high-grade white cardboard, most commonly made by pasting together sheets of heavy ledger paper."@en,
        "Een basismateriaal bestaande uit een hoogwaardig wit karton, meestal gemaakt door vellen zwaar registerpapier aan elkaar te plakken."@nl,
        "由陶土经超级压光或厚帐薄纸粘贴而成的上等白色纸板构成的基底材料。"@zh ;
    skos:inScheme <http://rdaregistry.info/termList/RDAMaterial> ;
    skos:prefLabel "Bristolkarton"@de,
        "Bristol board"@en,
        "cartulina brístol"@es,
        "bristol"@fr,
        "bristolkarton"@nl,
        "Bristol board"@sv,
        "上等纸板/布里斯托纸板"@zh .

<http://rdaregistry.info/termList/RDAMaterial/1005> a skos:Concept ;
    rdakit:toolkitDefinition "Ein Trägermaterial, das aus einem dicht gewebten Gewebe besteht, das in verschiedenen Stärken, normalerweise aus Flachs, Hanf, Jute oder Baumwolle gemacht wird, das als Unterlage für ein Ölgemälde verwendet wird. Oder ein locker gewebtes, gitterähnliches Gewebe, normalerweise aus Flachs, Hanf, Jute oder Baumwolle, das als Grundlage für die Gobelinstickerei verwendet wird."@de,
        "A material consisting of a closely woven textile made in various weights, usually of flax, hemp, jute, or cotton, used as a support for painting or printing; or a loosely woven, lattice-like mesh, usually of flax, hemp, jute, or cotton, used as a needlepoint foundation."@en,
        "Een basismateriaal bestaande uit nauw geweven textiel in diverse gewichten, meestal van vlas, hennep, jute of katoen, gebruikt als drager voor schilderen of drukken; of een losjes geweven, rasterachtig gaasdoek, meestal van vlas, hennep, jute of katoen, gebruikt als basis voor borduurwerk."@nl,
        "一般由不同重量的织物亚麻、大麻或棉花紧密编织用于绘画或印刷品支撑物，或由亚麻、大麻或棉花松散编织的网眼织物用于针绣基础的基底材料。"@zh ;
    rdakit:toolkitLabel "Leinwand"@de,
        "canvas"@en,
        "lona"@es,
        "canevas"@fr,
        "canvas"@nl,
        "målarduk"@sv,
        "帆布"@zh ;
    reg:identifier <http://metadataregistry.org/concepts/8459> ;
    reg:status <http://metadataregistry.org/uri/RegStatus/1001> ;
    skos:definition "Ein Trägermaterial, das aus einem dicht gewebten Gewebe besteht, das in verschiedenen Stärken, normalerweise aus Flachs, Hanf, Jute oder Baumwolle gemacht wird, das als Unterlage für ein Ölgemälde verwendet wird. Oder ein locker gewebtes, gitterähnliches Gewebe, normalerweise aus Flachs, Hanf, Jute oder Baumwolle, das als Grundlage für die Gobelinstickerei verwendet wird."@de,
        "A material consisting of a closely woven textile made in various weights, usually of flax, hemp, jute, or cotton, used as a support for painting or printing; or a loosely woven, lattice-like mesh, usually of flax, hemp, jute, or cotton, used as a needlepoint foundation."@en,
        "Een basismateriaal bestaande uit nauw geweven textiel in diverse gewichten, meestal van vlas, hennep, jute of katoen, gebruikt als drager voor schilderen of drukken; of een losjes geweven, rasterachtig gaasdoek, meestal van vlas, hennep, jute of katoen, gebruikt als basis voor borduurwerk."@nl,
        "一般由不同重量的织物亚麻、大麻或棉花紧密编织用于绘画或印刷品支撑物，或由亚麻、大麻或棉花松散编织的网眼织物用于针绣基础的基底材料。"@zh ;
    skos:inScheme <http://rdaregistry.info/termList/RDAMaterial> ;
    skos:prefLabel "Leinwand"@de,
        "canvas"@en,
        "lona"@es,
        "canevas"@fr,
        "canvas"@nl,
        "målarduk"@sv,
        "帆布"@zh .

<http://rdaregistry.info/termList/RDAMaterial/1006> a skos:Concept ;
    rdakit:toolkitDefinition "Ein Trägermaterial, das aus einer Art steifer Schichtpappe besteht, die dicker als 0,1524 Millimeter ist und typischerweise aus hochwertigem Zellstoff oder Altpappe besteht und sehr in Art und Stabilität variiert."@de,
        "A material consisting of a type of stiff sheet typically made of good-quality chemical pulp or rag pulp, varying greatly in type and strength, and that is thicker than 0.1524 mm."@en,
        "Een basismateriaal bestaande uit een soort stug vel, meestal gemaakt van goede kwaliteit chemische pulp of katoenpulp, in diverse soorten en stevigheid, dat dikker is dan 0,006 inches (0,15 mm)."@nl,
        "由厚于0.006英寸、不易弯曲的纸板构成的基底材料，通常由类型和稳定性不同的高质量化学纸浆或布纸板构成。"@zh ;
    rdakit:toolkitLabel "Karton"@de,
        "cardboard"@en,
        "cartón"@es,
        "carton"@fr,
        "bordkarton"@nl,
        "papp och kartong"@sv,
        "厚卡"@zh ;
    reg:identifier <http://metadataregistry.org/concepts/8460> ;
    reg:status <http://metadataregistry.org/uri/RegStatus/1001> ;
    skos:definition "Ein Trägermaterial, das aus einer Art steifer Schichtpappe besteht, die dicker als 0,1524 Millimeter ist und typischerweise aus hochwertigem Zellstoff oder Altpappe besteht und sehr in Art und Stabilität variiert."@de,
        "A material consisting of a type of stiff sheet typically made of good-quality chemical pulp or rag pulp, varying greatly in type and strength, and that is thicker than 0.1524 mm."@en,
        "Een basismateriaal bestaande uit een soort stug vel, meestal gemaakt van goede kwaliteit chemische pulp of katoenpulp, in diverse soorten en stevigheid, dat dikker is dan 0,006 inches (0,15 mm)."@nl,
        "由厚于0.006英寸、不易弯曲的纸板构成的基底材料，通常由类型和稳定性不同的高质量化学纸浆或布纸板构成。"@zh ;
    skos:inScheme <http://rdaregistry.info/termList/RDAMaterial> ;
    skos:prefLabel "Karton"@de,
        "cardboard"@en,
        "cartón"@es,
        "carton"@fr,
        "bordkarton"@nl,
        "papp och kartong"@sv,
        "厚卡"@zh .

<http://rdaregistry.info/termList/RDAMaterial/1007> a skos:Concept ;
    rdakit:toolkitDefinition "Ein Trägermaterial, das aus einem nichtmetallischen Mineral wie zum Beispiel Ton besteht, das bei hohen Temperaturen gebrannt wird, um ein hartes, zerbrechliches, hitze- und korrosionsbeständiges Material zu bilden."@de,
        "A material consisting of a nonmetallic mineral, such as clay, fired at a high temperature to form a hard, brittle, heat- and corrosion-resistant material."@en,
        "Een basismateriaal bestaande uit niet-metalen mineraal, zoals klei, op hoge temperatuur gebakken om een hard, broos, hittebestendig en roestvrij materiaal te verkrijgen."@nl,
        "由诸如黏土的非金属矿物经过高温烘烤形成坚硬、易碎、耐高温和腐蚀的材料构成的基底材料。"@zh ;
    rdakit:toolkitLabel "Keramik"@de,
        "ceramic"@en,
        "cerámica"@es,
        "céramique"@fr,
        "keramisch"@nl,
        "keramik"@sv,
        "陶"@zh ;
    reg:identifier <http://metadataregistry.org/concepts/8461> ;
    reg:status <http://metadataregistry.org/uri/RegStatus/1001> ;
    skos:definition "Ein Trägermaterial, das aus einem nichtmetallischen Mineral wie zum Beispiel Ton besteht, das bei hohen Temperaturen gebrannt wird, um ein hartes, zerbrechliches, hitze- und korrosionsbeständiges Material zu bilden."@de,
        "A material consisting of a nonmetallic mineral, such as clay, fired at a high temperature to form a hard, brittle, heat- and corrosion-resistant material."@en,
        "Een basismateriaal bestaande uit niet-metalen mineraal, zoals klei, op hoge temperatuur gebakken om een hard, broos, hittebestendig en roestvrij materiaal te verkrijgen."@nl,
        "由诸如黏土的非金属矿物经过高温烘烤形成坚硬、易碎、耐高温和腐蚀的材料构成的基底材料。"@zh ;
    skos:inScheme <http://rdaregistry.info/termList/RDAMaterial> ;
    skos:prefLabel "Keramik"@de,
        "ceramic"@en,
        "cerámica"@es,
        "céramique"@fr,
        "keramisch"@nl,
        "keramik"@sv,
        "陶"@zh .

<http://rdaregistry.info/termList/RDAMaterial/1008> a skos:Concept ;
    rdakit:toolkitDefinition "A material consisting of fine-grained limestone, or a soft, earthy form of calcium carbonate."@en ;
    rdakit:toolkitLabel "chalk"@en ;
    reg:identifier <http://metadataregistry.org/concepts/8462> ;
    reg:status <http://metadataregistry.org/uri/RegStatus/1001> ;
    skos:definition "A material consisting of fine-grained limestone, or a soft, earthy form of calcium carbonate."@en ;
    skos:inScheme <http://rdaregistry.info/termList/RDAMaterial> ;
    skos:prefLabel "chalk"@en .

<http://rdaregistry.info/termList/RDAMaterial/1009> a skos:Concept ;
    rdakit:toolkitDefinition "A material consisting of the dark grey residue made of carbon, and any remaining ash, obtained by removing water and other volatile constituents from animal and plant substances."@en ;
    rdakit:toolkitLabel "charcoal"@en ;
    reg:identifier <http://metadataregistry.org/concepts/8463> ;
    reg:status <http://metadataregistry.org/uri/RegStatus/1001> ;
    skos:definition "A material consisting of the dark grey residue made of carbon, and any remaining ash, obtained by removing water and other volatile constituents from animal and plant substances."@en ;
    skos:inScheme <http://rdaregistry.info/termList/RDAMaterial> ;
    skos:prefLabel "charcoal"@en .

<http://rdaregistry.info/termList/RDAMaterial/1011> a skos:Concept ;
    rdakit:toolkitDefinition "A material consisting of a coloured substance dissolved or suspended in a liquid that can be absorbed by the base material."@en ;
    rdakit:toolkitLabel "dye"@en ;
    reg:identifier <http://metadataregistry.org/concepts/8465> ;
    reg:status <http://metadataregistry.org/uri/RegStatus/1001> ;
    skos:definition "A material consisting of a coloured substance dissolved or suspended in a liquid that can be absorbed by the base material."@en ;
    skos:inScheme <http://rdaregistry.info/termList/RDAMaterial> ;
    skos:prefLabel "dye"@en .

<http://rdaregistry.info/termList/RDAMaterial/1012> a skos:Concept ;
    rdakit:toolkitDefinition "Ein Trägermaterial, das aus Siliciumdioxid (Quarz) verschmolzen mit einem basischen Oxid besteht; ist im Allgemeinen durchsichtig, aber oft durchscheinend oder undurchsichtig."@de,
        "A material consisting of silicon dioxide, known as silica, fused with one or more basic oxides; generally transparent but often translucent or opaque."@en,
        "Een basismateriaal bestaande uit siliciumdioxide (silica) in een synthese met één of meer basische oxiden; meestal transparent maar vaak doorschijnend of ondoorzichtig."@nl,
        "由二氧化硅与一种或多种碱性氧化物熔融在一起形成的基底材料，通常为透明，也常常为半透明或不透明。"@zh ;
    rdakit:toolkitLabel "Glas"@de,
        "glass"@en,
        "vidrio"@es,
        "verre"@fr,
        "glas"@nl,
        "玻璃"@zh ;
    reg:identifier <http://metadataregistry.org/concepts/8466> ;
    reg:status <http://metadataregistry.org/uri/RegStatus/1001> ;
    skos:definition "Ein Trägermaterial, das aus Siliciumdioxid (Quarz) verschmolzen mit einem basischen Oxid besteht; ist im Allgemeinen durchsichtig, aber oft durchscheinend oder undurchsichtig."@de,
        "A material consisting of silicon dioxide, known as silica, fused with one or more basic oxides; generally transparent but often translucent or opaque."@en,
        "Een basismateriaal bestaande uit siliciumdioxide (silica) in een synthese met één of meer basische oxiden; meestal transparent maar vaak doorschijnend of ondoorzichtig."@nl,
        "由二氧化硅与一种或多种碱性氧化物熔融在一起形成的基底材料，通常为透明，也常常为半透明或不透明。"@zh ;
    skos:inScheme <http://rdaregistry.info/termList/RDAMaterial> ;
    skos:prefLabel "Glas"@de,
        "glass"@en,
        "vidrio"@es,
        "verre"@fr,
        "glas"@nl,
        "玻璃"@zh .

<http://rdaregistry.info/termList/RDAMaterial/1013> a skos:Concept ;
    rdakit:toolkitDefinition "A material consisting of pigment and a binding substance, and sometimes added inert materials, to form an opaque, coloured, water-soluble paint."@en ;
    rdakit:toolkitLabel "gouache"@en ;
    reg:identifier <http://metadataregistry.org/concepts/8467> ;
    reg:status <http://metadataregistry.org/uri/RegStatus/1001> ;
    skos:definition "A material consisting of pigment and a binding substance, and sometimes added inert materials, to form an opaque, coloured, water-soluble paint."@en ;
    skos:inScheme <http://rdaregistry.info/termList/RDAMaterial> ;
    skos:prefLabel "gouache"@en ;
    skos:scopeNote "Poster paints are included. The term originally referred to the technique of oil paint applied on top of tempera."@en .

<http://rdaregistry.info/termList/RDAMaterial/1014> a skos:Concept ;
    rdakit:toolkitDefinition "A material consisting of a naturally occurring allotrope of carbon which is opaque, soft, greasy to the touch, and iron black to steel gray in color."@en ;
    rdakit:toolkitLabel "graphite"@en ;
    reg:identifier <http://metadataregistry.org/concepts/8468> ;
    reg:status <http://metadataregistry.org/uri/RegStatus/1001> ;
    skos:definition "A material consisting of a naturally occurring allotrope of carbon which is opaque, soft, greasy to the touch, and iron black to steel gray in color."@en ;
    skos:inScheme <http://rdaregistry.info/termList/RDAMaterial> ;
    skos:prefLabel "graphite"@en ;
    skos:scopeNote "The material is used in the form of powder, sticks, or in pencils."@en .

<http://rdaregistry.info/termList/RDAMaterial/1015> a skos:Concept ;
    rdakit:toolkitDefinition "Ein Trägermaterial, das aus irgendeiner festen, dichten, nicht biegsamen Platte besteht, die häufig aus Fasern hergestellt wird, die mit Hitze und Druck in einer heißen Presse miteinander verbunden werden."@de,
        "A material consisting of any firm, dense, rigid board, often manufactured from fiber consolidated in a hot press."@en,
        "Een basismateriaal bestaande uit elk stevig, compact en stijf plaatmateriaal, vaak vervaardigd uit vezels samengevoegd in een hete pers."@nl,
        "由通常经高温压制的纤维制成的紧实、高密度、刚硬的纸板构成的基底材料。"@zh ;
    rdakit:toolkitLabel "Hartfaserplatte"@de,
        "hardboard"@en,
        "tablero"@es,
        "panneau de fibres"@fr,
        "hardboard"@nl,
        "hårdpapp"@sv,
        "硬纸板"@zh ;
    reg:identifier <http://metadataregistry.org/concepts/8469> ;
    reg:status <http://metadataregistry.org/uri/RegStatus/1001> ;
    skos:altLabel "fibreboard"@en,
        "harde vezelplaat"@nl,
        "纤维板"@zh ;
    skos:definition "Ein Trägermaterial, das aus irgendeiner festen, dichten, nicht biegsamen Platte besteht, die häufig aus Fasern hergestellt wird, die mit Hitze und Druck in einer heißen Presse miteinander verbunden werden."@de,
        "A material consisting of any firm, dense, rigid board, often manufactured from fiber consolidated in a hot press."@en,
        "Een basismateriaal bestaande uit elk stevig, compact en stijf plaatmateriaal, vaak vervaardigd uit vezels samengevoegd in een hete pers."@nl,
        "由通常经高温压制的纤维制成的紧实、高密度、刚硬的纸板构成的基底材料。"@zh ;
    skos:inScheme <http://rdaregistry.info/termList/RDAMaterial> ;
    skos:prefLabel "Hartfaserplatte"@de,
        "hardboard"@en,
        "tablero"@es,
        "panneau de fibres"@fr,
        "hardboard"@nl,
        "hårdpapp"@sv,
        "硬纸板"@zh .

<http://rdaregistry.info/termList/RDAMaterial/1016> a skos:Concept ;
    rdakit:toolkitDefinition "A material consisting of laminated paper board that has paper layers glued to its surface."@en,
        "Een basismateriaal bestaande uit gelamineerd karton waarbij lagen papier geplakt zijn op het oppervlak; meestal gebruikt als tijdelijke drager voor kunstenaars."@nl,
        "由表面覆纸的层压纸板构成的基底材料，通常用作艺术家临时性的支撑物。"@zh ;
    rdakit:toolkitLabel "Zeichenkarton"@de,
        "illustration board"@en,
        "tablero gráfico"@es,
        "carton à dessiner"@fr,
        "illustratiekarton"@nl,
        "illustration board"@sv,
        "插图用纸板"@zh ;
    reg:identifier <http://metadataregistry.org/concepts/8470> ;
    reg:status <http://metadataregistry.org/uri/RegStatus/1001> ;
    skos:definition "A material consisting of laminated paper board that has paper layers glued to its surface."@en,
        "Een basismateriaal bestaande uit gelamineerd karton waarbij lagen papier geplakt zijn op het oppervlak; meestal gebruikt als tijdelijke drager voor kunstenaars."@nl,
        "由表面覆纸的层压纸板构成的基底材料，通常用作艺术家临时性的支撑物。"@zh ;
    skos:inScheme <http://rdaregistry.info/termList/RDAMaterial> ;
    skos:prefLabel "Zeichenkarton"@de,
        "illustration board"@en,
        "tablero gráfico"@es,
        "carton à dessiner"@fr,
        "illustratiekarton"@nl,
        "illustration board"@sv,
        "插图用纸板"@zh .

<http://rdaregistry.info/termList/RDAMaterial/1017> a skos:Concept ;
    rdakit:toolkitDefinition "A material consisting of pigment or dye contained in a liquid or paste."@en ;
    rdakit:toolkitLabel "ink"@en ;
    reg:identifier <http://metadataregistry.org/concepts/8471> ;
    reg:status <http://metadataregistry.org/uri/RegStatus/1001> ;
    skos:definition "A material consisting of pigment or dye contained in a liquid or paste."@en ;
    skos:inScheme <http://rdaregistry.info/termList/RDAMaterial> ;
    skos:prefLabel "ink"@en .

<http://rdaregistry.info/termList/RDAMaterial/1018> a skos:Concept ;
    rdakit:toolkitDefinition "Ein Trägermaterial, das aus dem Zahnbein besteht, das die Masse der Zähne und Stoßzähne von Tieren wie Elefanten, Walrosse und Narwalen formt."@de,
        "A material consisting of the dentine forming the bulk of the teeth and tusks of animals such as elephants, walruses, and narwhals."@en,
        "Een basismateriaal bestaande uit de dentine dat het merendeel vormt van de tanden en slagtanden van dieren zoals olifanten, walrussen en narwals."@nl,
        "由诸如大象、海象和独角鲸等动物牙齿和长牙主要部分的齿状物构成的基底材料。"@zh ;
    rdakit:toolkitLabel "Elfenbein"@de,
        "ivory"@en,
        "marfil"@es,
        "ivoire"@fr,
        "ivoor"@nl,
        "elfenben"@sv,
        "象牙"@zh ;
    reg:identifier <http://metadataregistry.org/concepts/8472> ;
    reg:status <http://metadataregistry.org/uri/RegStatus/1001> ;
    skos:definition "Ein Trägermaterial, das aus dem Zahnbein besteht, das die Masse der Zähne und Stoßzähne von Tieren wie Elefanten, Walrosse und Narwalen formt."@de,
        "A material consisting of the dentine forming the bulk of the teeth and tusks of animals such as elephants, walruses, and narwhals."@en,
        "Een basismateriaal bestaande uit de dentine dat het merendeel vormt van de tanden en slagtanden van dieren zoals olifanten, walrussen en narwals."@nl,
        "由诸如大象、海象和独角鲸等动物牙齿和长牙主要部分的齿状物构成的基底材料。"@zh ;
    skos:inScheme <http://rdaregistry.info/termList/RDAMaterial> ;
    skos:prefLabel "Elfenbein"@de,
        "ivory"@en,
        "marfil"@es,
        "ivoire"@fr,
        "ivoor"@nl,
        "elfenben"@sv,
        "象牙"@zh .

<http://rdaregistry.info/termList/RDAMaterial/1019> a skos:Concept ;
    rdakit:toolkitDefinition "A material generally used as a finish that may be clear or coloured, consisting of polymers or acrylic compounds dissolved in volatile organic compounds or other solvents, that when dry is a hard and durable material."@en ;
    rdakit:toolkitLabel "lacquer"@en ;
    reg:identifier <http://metadataregistry.org/concepts/8473> ;
    reg:status <http://metadataregistry.org/uri/RegStatus/1001> ;
    skos:definition "A material generally used as a finish that may be clear or coloured, consisting of polymers or acrylic compounds dissolved in volatile organic compounds or other solvents, that when dry is a hard and durable material."@en ;
    skos:inScheme <http://rdaregistry.info/termList/RDAMaterial> ;
    skos:prefLabel "lacquer"@en .

<http://rdaregistry.info/termList/RDAMaterial/1021> a skos:Concept ;
    rdakit:toolkitDefinition "A material that is a natural or synthetic inorganic compound consisting of particles that are highly magnetic and are commonly used to store binary or analog information."@en ;
    rdakit:toolkitLabel "magnetic particles"@en ;
    reg:identifier <http://metadataregistry.org/concepts/8475> ;
    reg:status <http://metadataregistry.org/uri/RegStatus/1001> ;
    skos:definition "A material that is a natural or synthetic inorganic compound consisting of particles that are highly magnetic and are commonly used to store binary or analog information."@en ;
    skos:inScheme <http://rdaregistry.info/termList/RDAMaterial> ;
    skos:prefLabel "magnetic particles"@en .

<http://rdaregistry.info/termList/RDAMaterial/1022> a skos:Concept ;
    rdakit:toolkitDefinition "Ein Trägermaterial, das aus einer Substanz besteht, die sich dadurch auszeichnet, dass sie ein guter Leiter von Strom und Wärme ist, undurchsichtig mit einem charakteristischem Schimmer ist, schmelzbar und normalerweise zu schmieden und zu verformen ist."@de,
        "A material consisting of a substance typified by being a good conductor of electricity and heat, opaque with a characteristic lustre, fusible, and usually malleable or ductile."@en,
        "Een basismateriaal bestaande uit een substantie waarvan het kenmerkend is dat deze elektriciteit en warmte goed geleidt, ondoorzichtig met een kenmerkende glans, smeltbaar en meestal smeedbaar of buigbaar."@nl,
        "由电热的良导体并具有特别光泽、易熔、可锻或可塑的不透明物质构成的基底材料。"@zh ;
    rdakit:toolkitLabel "Metall"@de,
        "metal"@en,
        "metal"@es,
        "métal"@fr,
        "metaal"@nl,
        "metall"@sv,
        "金属"@zh ;
    reg:identifier <http://metadataregistry.org/concepts/8476> ;
    reg:status <http://metadataregistry.org/uri/RegStatus/1001> ;
    skos:definition "Ein Trägermaterial, das aus einer Substanz besteht, die sich dadurch auszeichnet, dass sie ein guter Leiter von Strom und Wärme ist, undurchsichtig mit einem charakteristischem Schimmer ist, schmelzbar und normalerweise zu schmieden und zu verformen ist."@de,
        "A material consisting of a substance typified by being a good conductor of electricity and heat, opaque with a characteristic lustre, fusible, and usually malleable or ductile."@en,
        "Een basismateriaal bestaande uit een substantie waarvan het kenmerkend is dat deze elektriciteit en warmte goed geleidt, ondoorzichtig met een kenmerkende glans, smeltbaar en meestal smeedbaar of buigbaar."@nl,
        "由电热的良导体并具有特别光泽、易熔、可锻或可塑的不透明物质构成的基底材料。"@zh ;
    skos:inScheme <http://rdaregistry.info/termList/RDAMaterial> ;
    skos:prefLabel "Metall"@de,
        "metal"@en,
        "metal"@es,
        "métal"@fr,
        "metaal"@nl,
        "metall"@sv,
        "金属"@zh .

<http://rdaregistry.info/termList/RDAMaterial/1024> a skos:Concept ;
    rdakit:toolkitDefinition "A material consisting of pigment suspended in a drying oil."@en ;
    rdakit:toolkitLabel "oil paint"@en ;
    reg:identifier <http://metadataregistry.org/concepts/8478> ;
    reg:status <http://metadataregistry.org/uri/RegStatus/1001> ;
    skos:definition "A material consisting of pigment suspended in a drying oil."@en ;
    skos:inScheme <http://rdaregistry.info/termList/RDAMaterial> ;
    skos:prefLabel "oil paint"@en .

<http://rdaregistry.info/termList/RDAMaterial/1025> a skos:Concept ;
    rdakit:toolkitDefinition "Ein Trägermaterial, das aus dünner Materie oder gefalteten Blättern oder Gewebe von tierischen, pflanzlichen, mineralischen oder sythentischen Fasern besteht, das nach Auflösung in Wasser geformt und getrocknet wurde."@de,
        "A material consisting of thin material made from felted sheets or webs of animal, plant, mineral, or synthetic fibres formed and dried from a suspension in water."@en,
        "Een basismateriaal bestaande uit dun materiaal gemaakt van samengeperste vellen of weefsel van dierlijke, plantaardige, minerale of synthetische vezels, gevormd en gedroogd na onderdompeling in water."@nl,
        "由动物、植物、矿物或合成纤维粘结成的张或网经水中悬浮后成形并晒干制成的薄的材料构成的基底材料。"@zh ;
    rdakit:toolkitLabel "Papier"@de,
        "paper"@en,
        "papel"@es,
        "papier"@fr,
        "papier"@nl,
        "papper"@sv,
        "纸"@zh ;
    reg:identifier <http://metadataregistry.org/concepts/8479> ;
    reg:status <http://metadataregistry.org/uri/RegStatus/1001> ;
    skos:definition "Ein Trägermaterial, das aus dünner Materie oder gefalteten Blättern oder Gewebe von tierischen, pflanzlichen, mineralischen oder sythentischen Fasern besteht, das nach Auflösung in Wasser geformt und getrocknet wurde."@de,
        "A material consisting of thin material made from felted sheets or webs of animal, plant, mineral, or synthetic fibres formed and dried from a suspension in water."@en,
        "Een basismateriaal bestaande uit dun materiaal gemaakt van samengeperste vellen of weefsel van dierlijke, plantaardige, minerale of synthetische vezels, gevormd en gedroogd na onderdompeling in water."@nl,
        "由动物、植物、矿物或合成纤维粘结成的张或网经水中悬浮后成形并晒干制成的薄的材料构成的基底材料。"@zh ;
    skos:inScheme <http://rdaregistry.info/termList/RDAMaterial> ;
    skos:prefLabel "Papier"@de,
        "paper"@en,
        "papel"@es,
        "papier"@fr,
        "papier"@nl,
        "papper"@sv,
        "纸"@zh .

<http://rdaregistry.info/termList/RDAMaterial/1027> a skos:Concept ;
    rdakit:toolkitDefinition "A material consisting of pigment mixed with a binder, usually in the form of a stick."@en ;
    rdakit:toolkitLabel "pastel"@en ;
    reg:identifier <http://metadataregistry.org/concepts/8481> ;
    reg:status <http://metadataregistry.org/uri/RegStatus/1001> ;
    skos:definition "A material consisting of pigment mixed with a binder, usually in the form of a stick."@en ;
    skos:inScheme <http://rdaregistry.info/termList/RDAMaterial> ;
    skos:prefLabel "pastel"@en .

<http://rdaregistry.info/termList/RDAMaterial/1028> a skos:Concept ;
    rdakit:toolkitDefinition "Ein Trägermaterial, das aus einem Puder besteht, der aus Kalziumsulfatdihydrat (Gips) oder Kalziumkarbonat gemischt mit Wasser sowie manchmal einem Füllstoff hergestellt wird, um eine Paste zu bilden, die Wärme freisetzt und dann aushärtet."@de,
        "A material consisting of a powder prepared from calcium sulphate dihydrate, known as gypsum, or calcium carbonate and mixed with water and sometimes a filler to form a paste that liberates heat and then hardens."@en,
        "Een bevestigd materiaal of basismateriaal bestaande uit een poeder bereid uit calciumsulfaatdihydraat (gips) en calciumcarbonaat en gemengd met water en soms een vulmiddel om een smeersel te vormen dat warmte afgeeft en dan hard wordt."@nl,
        "由二水硫酸钙（石膏）或碳酸钙粉末与水，有时也与填料混合而成的膏状物经热量释放后变硬，从而构成的应用材料或基底材料。"@zh ;
    rdakit:toolkitLabel "Gips"@de,
        "plaster"@en,
        "yeso"@es,
        "plâtre"@fr,
        "pleister"@nl,
        "gips"@sv,
        "石膏"@zh ;
    reg:identifier <http://metadataregistry.org/concepts/8482> ;
    reg:status <http://metadataregistry.org/uri/RegStatus/1001> ;
    skos:definition "Ein Trägermaterial, das aus einem Puder besteht, der aus Kalziumsulfatdihydrat (Gips) oder Kalziumkarbonat gemischt mit Wasser sowie manchmal einem Füllstoff hergestellt wird, um eine Paste zu bilden, die Wärme freisetzt und dann aushärtet."@de,
        "A material consisting of a powder prepared from calcium sulphate dihydrate, known as gypsum, or calcium carbonate and mixed with water and sometimes a filler to form a paste that liberates heat and then hardens."@en,
        "Een bevestigd materiaal of basismateriaal bestaande uit een poeder bereid uit calciumsulfaatdihydraat (gips) en calciumcarbonaat en gemengd met water en soms een vulmiddel om een smeersel te vormen dat warmte afgeeft en dan hard wordt."@nl,
        "由二水硫酸钙（石膏）或碳酸钙粉末与水，有时也与填料混合而成的膏状物经热量释放后变硬，从而构成的应用材料或基底材料。"@zh ;
    skos:inScheme <http://rdaregistry.info/termList/RDAMaterial> ;
    skos:prefLabel "Gips"@de,
        "plaster"@en,
        "yeso"@es,
        "plâtre"@fr,
        "pleister"@nl,
        "gips"@sv,
        "石膏"@zh .

<http://rdaregistry.info/termList/RDAMaterial/1031> a skos:Concept ;
    rdakit:toolkitDefinition "Ein Trägermaterial, das aus einem feuerfesten weißen Ton (Kaolin) und einem feldspathaltigen Stein besteht, die erhitzt werden, um ein keramisches Material zu bilden."@de,
        "A material consisting of a refractory white clay, known as kaolin, and a feldspathic rock that is heated to form a ceramic material."@en,
        "Een basismateriaal bestaande uit een vuurvaste witte klei (porseleinaarde) en een veldspaten steen die verhit wordt om een keramisch materiaal te vormen."@nl,
        "由耐火的白色黏土（高岭土）和长石岩经高温烧制成的陶瓷材料构成的应用材料。"@zh ;
    rdakit:toolkitLabel "Porzellan"@de,
        "porcelain"@en,
        "porcelana"@es,
        "porcelaine"@fr,
        "porselein"@nl,
        "瓷"@zh ;
    reg:identifier <http://metadataregistry.org/concepts/8485> ;
    reg:status <http://metadataregistry.org/uri/RegStatus/1001> ;
    skos:definition "Ein Trägermaterial, das aus einem feuerfesten weißen Ton (Kaolin) und einem feldspathaltigen Stein besteht, die erhitzt werden, um ein keramisches Material zu bilden."@de,
        "A material consisting of a refractory white clay, known as kaolin, and a feldspathic rock that is heated to form a ceramic material."@en,
        "Een basismateriaal bestaande uit een vuurvaste witte klei (porseleinaarde) en een veldspaten steen die verhit wordt om een keramisch materiaal te vormen."@nl,
        "由耐火的白色黏土（高岭土）和长石岩经高温烧制成的陶瓷材料构成的应用材料。"@zh ;
    skos:inScheme <http://rdaregistry.info/termList/RDAMaterial> ;
    skos:prefLabel "Porzellan"@de,
        "porcelain"@en,
        "porcelana"@es,
        "porcelaine"@fr,
        "porselein"@nl,
        "瓷"@zh .

<http://rdaregistry.info/termList/RDAMaterial/1032> a skos:Concept ;
    rdakit:toolkitDefinition "A material consisting of natural or synthetic polymers that have a high degree of resilience and elasticity."@en,
        "Een basismateriaal bestaande uit natuurlijke of synthetische polymeren die een hoge graad van weerstand en elasticiteit hebben."@nl,
        "由具有高还原力和弹性的自然或合成聚合物构成的基底材料。"@zh ;
    rdakit:toolkitLabel "rubber"@en,
        "rubber"@nl,
        "gummi"@sv,
        "橡胶"@zh ;
    reg:identifier <http://metadataregistry.org/concepts/8486> ;
    reg:status <http://metadataregistry.org/uri/RegStatus/1001> ;
    skos:definition "A material consisting of natural or synthetic polymers that have a high degree of resilience and elasticity."@en,
        "Een basismateriaal bestaande uit natuurlijke of synthetische polymeren die een hoge graad van weerstand en elasticiteit hebben."@nl,
        "由具有高还原力和弹性的自然或合成聚合物构成的基底材料。"@zh ;
    skos:inScheme <http://rdaregistry.info/termList/RDAMaterial> ;
    skos:prefLabel "rubber"@en,
        "rubber"@nl,
        "gummi"@sv,
        "橡胶"@zh .

<http://rdaregistry.info/termList/RDAMaterial/1034> a skos:Concept ;
    rdakit:toolkitDefinition "Ein Trägermaterial, das aus Lackharz besteht, einer harzhaltigen Substanz, die von der weiblichen Lackschildlaus ausgeschieden wird, die in Ethylalkohol gelöst werden kann, um eine Flüssigkeit zu bilden, die mit einem Pinsel aufgetragen werden kann."@de,
        "A material consisting of lac, a resinous substance excreted by the female lac insect, that can be dissolved in ethyl alcohol to form a liquid that can be applied with a brush."@en,
        "Een basismateriaal bestaande uit lak, een harsachtige substantie uitgescheiden door vrouwtjes lakinsecten, dat opgelost kan worden in ethylalcohol om een vloeistof te vormen die aangebracht kan worden met een kwast."@nl,
        "由紫胶虫雌虫分泌的、溶解于乙醇后形成的液体可用刷子蘸取的紫胶（树脂状物质）构成的基底材料。"@zh ;
    rdakit:toolkitLabel "Schellack"@de,
        "shellac"@en,
        "laca"@es,
        "gomme laque"@fr,
        "schellak"@nl,
        "shellack"@sv,
        "虫胶"@zh ;
    reg:identifier <http://metadataregistry.org/concepts/8488> ;
    reg:status <http://metadataregistry.org/uri/RegStatus/1001> ;
    skos:definition "Ein Trägermaterial, das aus Lackharz besteht, einer harzhaltigen Substanz, die von der weiblichen Lackschildlaus ausgeschieden wird, die in Ethylalkohol gelöst werden kann, um eine Flüssigkeit zu bilden, die mit einem Pinsel aufgetragen werden kann."@de,
        "A material consisting of lac, a resinous substance excreted by the female lac insect, that can be dissolved in ethyl alcohol to form a liquid that can be applied with a brush."@en,
        "Een basismateriaal bestaande uit lak, een harsachtige substantie uitgescheiden door vrouwtjes lakinsecten, dat opgelost kan worden in ethylalcohol om een vloeistof te vormen die aangebracht kan worden met een kwast."@nl,
        "由紫胶虫雌虫分泌的、溶解于乙醇后形成的液体可用刷子蘸取的紫胶（树脂状物质）构成的基底材料。"@zh ;
    skos:inScheme <http://rdaregistry.info/termList/RDAMaterial> ;
    skos:prefLabel "Schellack"@de,
        "shellac"@en,
        "laca"@es,
        "gomme laque"@fr,
        "schellak"@nl,
        "shellack"@sv,
        "虫胶"@zh .

<http://rdaregistry.info/termList/RDAMaterial/1036> a skos:Concept ;
    rdakit:toolkitDefinition "Ein Trägermaterial, das aus Gestein in seiner natürlich vorkommenden Form besteht oder gestaltet, zerkleinert oder auf andere Art und Weise geformt wurde."@de,
        "A material consisting of rock in its naturally occurring shape or that has been cut, shaped, crushed, or otherwise formed."@en,
        "Een basismateriaal bestaande uit steen in de natuurlijk voorkomende vorm al dan niet gesneden, geslepen, verpulverd of anderszins gevormd."@nl,
        "由自然形状或经过切割、塑形、碾压或其他方式成形的岩石构成的基底材料。"@zh ;
    rdakit:toolkitLabel "Stein"@de,
        "stone"@en,
        "piedra"@es,
        "pierre"@fr,
        "steen"@nl,
        "sten"@sv,
        "石"@zh ;
    reg:identifier <http://metadataregistry.org/concepts/8490> ;
    reg:status <http://metadataregistry.org/uri/RegStatus/1001> ;
    skos:definition "Ein Trägermaterial, das aus Gestein in seiner natürlich vorkommenden Form besteht oder gestaltet, zerkleinert oder auf andere Art und Weise geformt wurde."@de,
        "A material consisting of rock in its naturally occurring shape or that has been cut, shaped, crushed, or otherwise formed."@en,
        "Een basismateriaal bestaande uit steen in de natuurlijk voorkomende vorm al dan niet gesneden, geslepen, verpulverd of anderszins gevormd."@nl,
        "由自然形状或经过切割、塑形、碾压或其他方式成形的岩石构成的基底材料。"@zh ;
    skos:inScheme <http://rdaregistry.info/termList/RDAMaterial> ;
    skos:prefLabel "Stein"@de,
        "stone"@en,
        "piedra"@es,
        "pierre"@fr,
        "steen"@nl,
        "sten"@sv,
        "石"@zh .

<http://rdaregistry.info/termList/RDAMaterial/1037> a skos:Concept ;
    rdakit:toolkitDefinition "Ein Trägermaterial, das durch Verarbeitung von künstlich geschaffenen Materialien erzeugt wurde, normalerweise als Ersatz für ein natürliches Material."@de,
        "A material created by processing man-made materials, usually as a substitute for a natural material."@en,
        "由人造材料加工而成，通常作为自然材料替代品的基底材料。"@zh ;
    rdakit:toolkitLabel "Kunststoff"@de,
        "synthetic"@en,
        "sintético"@es,
        "matière synthétique"@fr,
        "syntetiskt material"@sv,
        "合成物"@zh ;
    reg:identifier <http://metadataregistry.org/concepts/8491> ;
    reg:status <http://metadataregistry.org/uri/RegStatus/1001> ;
    skos:definition "Ein Trägermaterial, das durch Verarbeitung von künstlich geschaffenen Materialien erzeugt wurde, normalerweise als Ersatz für ein natürliches Material."@de,
        "A material created by processing man-made materials, usually as a substitute for a natural material."@en,
        "由人造材料加工而成，通常作为自然材料替代品的基底材料。"@zh ;
    skos:inScheme <http://rdaregistry.info/termList/RDAMaterial> ;
    skos:prefLabel "Kunststoff"@de,
        "synthetic"@en,
        "sintético"@es,
        "matière synthétique"@fr,
        "syntetiskt material"@sv,
        "合成物"@zh .

<http://rdaregistry.info/termList/RDAMaterial/1038> a skos:Concept ;
    rdakit:toolkitDefinition "A material consisting of pigment mixed with a water-soluble binder medium, usually a glutinous material such as egg yolk or some other size, to form a permanent fast-drying painting medium."@en ;
    rdakit:toolkitLabel "tempera"@en ;
    reg:identifier <http://metadataregistry.org/concepts/8492> ;
    reg:status <http://metadataregistry.org/uri/RegStatus/1001> ;
    skos:definition "A material consisting of pigment mixed with a water-soluble binder medium, usually a glutinous material such as egg yolk or some other size, to form a permanent fast-drying painting medium."@en ;
    skos:inScheme <http://rdaregistry.info/termList/RDAMaterial> ;
    skos:prefLabel "tempera"@en .

<http://rdaregistry.info/termList/RDAMaterial/1039> a skos:Concept ;
    rdakit:toolkitDefinition "Ein Trägermaterial, das durch Weben, Filzen, Knoten, Zwirnen oder anderweitige BEarbeitung natürlicher oder sythetischer Fasern erzeugt wird, so dass sie zusammenhängen."@de,
        "A material produced by weaving, felting, knotting, twining, or otherwise processing natural or synthetic fibers so that they cohere."@en,
        "Een basismateriaal geproduceerd door weven, filten, knopen, vlechten of anderszins verwerken van natuurlijke of synthetische vezels zodat deze één geheel vormen."@nl,
        "将自然或合成纤维经过编织、毡合、打结、耦合或其他工序加工使其黏合构成的基底材料。"@zh ;
    rdakit:toolkitLabel "Gewebe"@de,
        "textile"@en,
        "textil"@es,
        "textile"@fr,
        "textiel"@nl,
        "textil"@sv,
        "织物"@zh ;
    reg:identifier <http://metadataregistry.org/concepts/8493> ;
    reg:status <http://metadataregistry.org/uri/RegStatus/1001> ;
    skos:definition "Ein Trägermaterial, das durch Weben, Filzen, Knoten, Zwirnen oder anderweitige BEarbeitung natürlicher oder sythetischer Fasern erzeugt wird, so dass sie zusammenhängen."@de,
        "A material produced by weaving, felting, knotting, twining, or otherwise processing natural or synthetic fibers so that they cohere."@en,
        "Een basismateriaal geproduceerd door weven, filten, knopen, vlechten of anderszins verwerken van natuurlijke of synthetische vezels zodat deze één geheel vormen."@nl,
        "将自然或合成纤维经过编织、毡合、打结、耦合或其他工序加工使其黏合构成的基底材料。"@zh ;
    skos:inScheme <http://rdaregistry.info/termList/RDAMaterial> ;
    skos:prefLabel "Gewebe"@de,
        "textile"@en,
        "textil"@es,
        "textile"@fr,
        "textiel"@nl,
        "textil"@sv,
        "织物"@zh ;
    skos:scopeNote "Excludes fibreboard, paper, papier-mâché, and papyrus."@en .

<http://rdaregistry.info/termList/RDAMaterial/1042> a skos:Concept ;
    rdakit:toolkitDefinition "Ein Trägermaterial, das aus einem Polymer oder einem Copolymer besteht, das aus einer Vinylgruppe (Ethenyl) abgeleitet wird, typischerweise Vinylchlorid."@de,
        "A material consisting of a polymer or copolymer derived from a vinyl group, typically vinyl chloride."@en,
        "Een basismateriaal bestaande uit een polymeer of co-polymeer afkomstig uit de vinylgroep (ethenyl), meestal vinylchloride."@nl,
        "由乙烯基群，尤其是氯乙烯派生而成的聚合物或共聚物构成的基底材料。"@zh ;
    rdakit:toolkitLabel "Vinyl"@de,
        "vinyl"@en,
        "vinilo"@es,
        "vinyle"@fr,
        "vinyl"@nl,
        "乙烯树脂"@zh ;
    reg:identifier <http://metadataregistry.org/concepts/8496> ;
    reg:status <http://metadataregistry.org/uri/RegStatus/1001> ;
    skos:definition "Ein Trägermaterial, das aus einem Polymer oder einem Copolymer besteht, das aus einer Vinylgruppe (Ethenyl) abgeleitet wird, typischerweise Vinylchlorid."@de,
        "A material consisting of a polymer or copolymer derived from a vinyl group, typically vinyl chloride."@en,
        "Een basismateriaal bestaande uit een polymeer of co-polymeer afkomstig uit de vinylgroep (ethenyl), meestal vinylchloride."@nl,
        "由乙烯基群，尤其是氯乙烯派生而成的聚合物或共聚物构成的基底材料。"@zh ;
    skos:inScheme <http://rdaregistry.info/termList/RDAMaterial> ;
    skos:prefLabel "Vinyl"@de,
        "vinyl"@en,
        "vinilo"@es,
        "vinyle"@fr,
        "vinyl"@nl,
        "乙烯树脂"@zh .

<http://rdaregistry.info/termList/RDAMaterial/1043> a skos:Concept ;
    rdakit:toolkitDefinition "A material consisting of pigment suspended in water to form a transparent painting medium."@en ;
    rdakit:toolkitLabel "watercolour"@en ;
    reg:identifier <http://metadataregistry.org/concepts/8497> ;
    reg:status <http://metadataregistry.org/uri/RegStatus/1001> ;
    skos:altLabel "watercolor"@en ;
    skos:definition "A material consisting of pigment suspended in water to form a transparent painting medium."@en ;
    skos:inScheme <http://rdaregistry.info/termList/RDAMaterial> ;
    skos:prefLabel "watercolour"@en .

<http://rdaregistry.info/termList/RDAMaterial/1044> a skos:Concept ;
    rdakit:toolkitDefinition "Ein Trägermaterial, das aus einer chemischen Komponente aus tierischer, pflanzliche, mineralischer oder synthetischer Quelle besteht, das bei Raumtemperatur verformbar, beim Berühren leicht ölig und normalerweise durchscheinend, Wasser abweisend und in organischen Lösemitteln auflösbar ist."@de,
        "A material consisting of a chemical compound from an animal, plant, mineral, or synthetic source that is malleable near ambient temperatures, slightly greasy to the touch, with a low melting point, and usually translucent, water-repellant, and soluble in organic solvents."@en,
        "Een bevestigd materiaal of basismateriaal bestaande uit een chemische samenstelling van dierlijke, plantaardige, minerale of synthetische bron die kneedbaar is bij omgevingstemperaturen, enigszins vettig is om aan te raken, met een laag smeltpunt, en meestal doorzichtig, waterafstotend en oplosbaar in organische oplosmiddelen."@nl,
        "由动物、植物、矿物或合成材料制成的，在环境温度中可塑、触感略微油腻、熔点低、通常为半透明、防水并溶于有机溶剂的化合物构成的应用材料或基底材料。"@zh ;
    rdakit:toolkitLabel "Wachs"@de,
        "wax"@en,
        "cera"@es,
        "cire"@fr,
        "was"@nl,
        "蜡"@zh ;
    reg:identifier <http://metadataregistry.org/concepts/8498> ;
    reg:status <http://metadataregistry.org/uri/RegStatus/1001> ;
    skos:definition "Ein Trägermaterial, das aus einer chemischen Komponente aus tierischer, pflanzliche, mineralischer oder synthetischer Quelle besteht, das bei Raumtemperatur verformbar, beim Berühren leicht ölig und normalerweise durchscheinend, Wasser abweisend und in organischen Lösemitteln auflösbar ist."@de,
        "A material consisting of a chemical compound from an animal, plant, mineral, or synthetic source that is malleable near ambient temperatures, slightly greasy to the touch, with a low melting point, and usually translucent, water-repellant, and soluble in organic solvents."@en,
        "Een bevestigd materiaal of basismateriaal bestaande uit een chemische samenstelling van dierlijke, plantaardige, minerale of synthetische bron die kneedbaar is bij omgevingstemperaturen, enigszins vettig is om aan te raken, met een laag smeltpunt, en meestal doorzichtig, waterafstotend en oplosbaar in organische oplosmiddelen."@nl,
        "由动物、植物、矿物或合成材料制成的，在环境温度中可塑、触感略微油腻、熔点低、通常为半透明、防水并溶于有机溶剂的化合物构成的应用材料或基底材料。"@zh ;
    skos:inScheme <http://rdaregistry.info/termList/RDAMaterial> ;
    skos:prefLabel "Wachs"@de,
        "wax"@en,
        "cera"@es,
        "cire"@fr,
        "was"@nl,
        "蜡"@zh .

<http://rdaregistry.info/termList/RDAMaterial/1045> a skos:Concept ;
    rdakit:toolkitDefinition "Ein Trägermaterial, das aus dem Hauptgewebe von Bäumen und ähnlichen Pflanzen besteht."@de,
        "A material consisting of the principal tissue of trees and similar plants."@en,
        "Een basismateriaal bestaande uit het voornaamste weefsel van bomen en vergelijkbare planten."@nl,
        "由树或相似植物的主要组织构成的基底材料。"@zh ;
    rdakit:toolkitLabel "Holz"@de,
        "wood"@en,
        "madera"@es,
        "bois"@fr,
        "hout"@nl,
        "木"@zh ;
    reg:identifier <http://metadataregistry.org/concepts/8499> ;
    reg:status <http://metadataregistry.org/uri/RegStatus/1001> ;
    skos:definition "Ein Trägermaterial, das aus dem Hauptgewebe von Bäumen und ähnlichen Pflanzen besteht."@de,
        "A material consisting of the principal tissue of trees and similar plants."@en,
        "Een basismateriaal bestaande uit het voornaamste weefsel van bomen en vergelijkbare planten."@nl,
        "由树或相似植物的主要组织构成的基底材料。"@zh ;
    skos:inScheme <http://rdaregistry.info/termList/RDAMaterial> ;
    skos:prefLabel "Holz"@de,
        "wood"@en,
        "madera"@es,
        "bois"@fr,
        "hout"@nl,
        "木"@zh .

<http://rdaregistry.info/termList/RDAMaterial/1046> a skos:Concept ;
    rdakit:toolkitDefinition "A material consisting of an emulsion of one or more light-sensitive layers of diazonium salts in a polyester or acetate base that react with dye couplers when processed to produce azo dye images."@en ;
    rdakit:toolkitLabel "diazo emulsion"@en ;
    reg:identifier <http://metadataregistry.org/concepts/8500> ;
    reg:status <http://metadataregistry.org/uri/RegStatus/1001> ;
    skos:definition "A material consisting of an emulsion of one or more light-sensitive layers of diazonium salts in a polyester or acetate base that react with dye couplers when processed to produce azo dye images."@en ;
    skos:inScheme <http://rdaregistry.info/termList/RDAMaterial> ;
    skos:prefLabel "diazo emulsion"@en ;
    skos:scopeNote "A material usually applied to the base material of a microfilm or microfiche."@en .

<http://rdaregistry.info/termList/RDAMaterial/1047> a skos:Concept ;
    rdakit:toolkitDefinition "A material consisting of an emulsion of a light-sensitive compound of silver and chlorine, bromine, iodine or fluorine suspended in a colloidal medium, usually gelatin."@en ;
    rdakit:toolkitLabel "silver halide emulsion"@en ;
    reg:identifier <http://metadataregistry.org/concepts/8501> ;
    reg:status <http://metadataregistry.org/uri/RegStatus/1001> ;
    skos:definition "A material consisting of an emulsion of a light-sensitive compound of silver and chlorine, bromine, iodine or fluorine suspended in a colloidal medium, usually gelatin."@en ;
    skos:inScheme <http://rdaregistry.info/termList/RDAMaterial> ;
    skos:prefLabel "silver halide emulsion"@en ;
    skos:scopeNote "A material usually applied to the base material of a microfilm or microfiche."@en .

<http://rdaregistry.info/termList/RDAMaterial/1048> a skos:Concept ;
    rdakit:toolkitDefinition "A material consisting of an emulsion of one or more light-sensitive layers of diazonium salts in a polyester thermoplastic base that decompose on exposure to produce nitrogen bubbles, known as vesicles, that form a latent image, commonly blue or beige, which becomes visible and fixed when heated and allowed to cool."@en ;
    rdakit:toolkitLabel "vesicular emulsion"@en ;
    reg:identifier <http://metadataregistry.org/concepts/8502> ;
    reg:status <http://metadataregistry.org/uri/RegStatus/1001> ;
    skos:definition "A material consisting of an emulsion of one or more light-sensitive layers of diazonium salts in a polyester thermoplastic base that decompose on exposure to produce nitrogen bubbles, known as vesicles, that form a latent image, commonly blue or beige, which becomes visible and fixed when heated and allowed to cool."@en ;
    skos:inScheme <http://rdaregistry.info/termList/RDAMaterial> ;
    skos:prefLabel "vesicular emulsion"@en ;
    skos:scopeNote "A material usually applied to the base material of a microfilm or microfiche."@en .

<http://rdaregistry.info/termList/RDAMaterial/1020> a skos:Concept ;
    rdakit:toolkitDefinition "Ein Trägermaterial, das aus der Haut oder dem Fell eines Tieres besteht, die/das gegerbt wird, um es gegen Fäulnis zu schützen, und relativ weich und flexibel ist, wenn es trocken ist."@de,
        "A material consisting of the skin or hide of an animal that has been tanned to render it resistant to putrefaction and relatively soft and flexible when dry."@en,
        "Een basismateriaal bestaande uit de huid of pels van een dier dat gelooid is om het weerbaar te maken tegen bederf en redelijk zacht en flexibel als deze droog is."@nl,
        "由经过硝皮使其干燥后不易腐烂并相对柔软有弹性的动物皮肤或皮毛构成的基底材料。"@zh ;
    rdakit:toolkitLabel "Leder"@de,
        "leather"@en,
        "cuero"@es,
        "cuir"@fr,
        "leer"@nl,
        "läder"@sv,
        "皮革"@zh ;
    reg:identifier <http://metadataregistry.org/concepts/8474> ;
    reg:status <http://metadataregistry.org/uri/RegStatus/1001> ;
    skos:definition "Ein Trägermaterial, das aus der Haut oder dem Fell eines Tieres besteht, die/das gegerbt wird, um es gegen Fäulnis zu schützen, und relativ weich und flexibel ist, wenn es trocken ist."@de,
        "A material consisting of the skin or hide of an animal that has been tanned to render it resistant to putrefaction and relatively soft and flexible when dry."@en,
        "Een basismateriaal bestaande uit de huid of pels van een dier dat gelooid is om het weerbaar te maken tegen bederf en redelijk zacht en flexibel als deze droog is."@nl,
        "由经过硝皮使其干燥后不易腐烂并相对柔软有弹性的动物皮肤或皮毛构成的基底材料。"@zh ;
    skos:inScheme <http://rdaregistry.info/termList/RDAMaterial> ;
    skos:prefLabel "Leder"@de,
        "leather"@en,
        "cuero"@es,
        "cuir"@fr,
        "leer"@nl,
        "läder"@sv,
        "皮革"@zh ;
    skos:related <http://rdaregistry.info/termList/RDAMaterial/1035> .

<http://rdaregistry.info/termList/RDAMaterial/1041> a skos:Concept ;
    rdakit:toolkitDefinition "Ein Trägermaterial, das aus Kalbs- oder Lammpergament von hoher Qualität besteht."@de,
        "A material consisting of fine-quality calf or lamb parchment."@en,
        "Een basismateriaal bestaande uit kalfs- of lamsperkament van verfijnde kwaliteit."@nl,
        "由高品质的小牛或羔羊皮纸构成的基底材料。"@zh ;
    rdakit:toolkitLabel "Vellum"@de,
        "vellum"@en,
        "vitela"@es,
        "vélin"@fr,
        "vellum"@nl,
        "牛皮纸"@zh ;
    reg:identifier <http://metadataregistry.org/concepts/8495> ;
    reg:status <http://metadataregistry.org/uri/RegStatus/1001> ;
    skos:definition "Ein Trägermaterial, das aus Kalbs- oder Lammpergament von hoher Qualität besteht."@de,
        "A material consisting of fine-quality calf or lamb parchment."@en,
        "Een basismateriaal bestaande uit kalfs- of lamsperkament van verfijnde kwaliteit."@nl,
        "由高品质的小牛或羔羊皮纸构成的基底材料。"@zh ;
    skos:inScheme <http://rdaregistry.info/termList/RDAMaterial> ;
    skos:prefLabel "Vellum"@de,
        "vellum"@en,
        "vitela"@es,
        "vélin"@fr,
        "vellum"@nl,
        "牛皮纸"@zh ;
    skos:related <http://rdaregistry.info/termList/RDAMaterial/1026> .

<http://rdaregistry.info/termList/RDAMaterial/1001> a skos:Concept ;
    rdakit:toolkitDefinition "A material composed of the acetate ester of cellulose."@en,
        "Een basismateriaal samengesteld uit de acetaat-ester van cellulose."@nl,
        "由纤维素醋酸酯组成的基底材料。"@zh ;
    rdakit:toolkitLabel "acetate"@en,
        "acetaat"@nl,
        "acetat"@sv,
        "醋酸纤维素"@zh ;
    reg:identifier <http://metadataregistry.org/concepts/8455> ;
    reg:status <http://metadataregistry.org/uri/RegStatus/1001> ;
    skos:altLabel "cellulose acetate"@en,
        "乙酸纤维素"@zh ;
    skos:definition "A material composed of the acetate ester of cellulose."@en,
        "Een basismateriaal samengesteld uit de acetaat-ester van cellulose."@nl,
        "由纤维素醋酸酯组成的基底材料。"@zh ;
    skos:inScheme <http://rdaregistry.info/termList/RDAMaterial> ;
    skos:prefLabel "acetate"@en,
        "acetaat"@nl,
        "acetat"@sv,
        "醋酸纤维素"@zh ;
    skos:related <http://rdaregistry.info/termList/RDAMaterial/1029>,
        <http://rdaregistry.info/termList/RDAMaterial/1040> .

<http://rdaregistry.info/termList/RDAMaterial/1023> a skos:Concept ;
    rdakit:toolkitDefinition "A material of cellulose nitrate plasticized with camphor."@en,
        "Een bevestigd materiaal of basismateriaal van cellulosenitraat geplastifiseerd met kamfer."@nl,
        "由经过莰酮塑化的硝化纤维应用材料或基底材料。"@zh ;
    rdakit:toolkitLabel "nitrate"@en,
        "nitraat"@nl,
        "nitrat"@sv,
        "硝酸纤维素"@zh ;
    reg:identifier <http://metadataregistry.org/concepts/8477> ;
    reg:status <http://metadataregistry.org/uri/RegStatus/1001> ;
    skos:altLabel "celluloid"@en,
        "celluloid"@nl,
        "赛璐珞"@zh ;
    skos:definition "A material of cellulose nitrate plasticized with camphor."@en,
        "Een bevestigd materiaal of basismateriaal van cellulosenitraat geplastifiseerd met kamfer."@nl,
        "由经过莰酮塑化的硝化纤维应用材料或基底材料。"@zh ;
    skos:inScheme <http://rdaregistry.info/termList/RDAMaterial> ;
    skos:prefLabel "nitrate"@en,
        "nitraat"@nl,
        "nitrat"@sv,
        "硝酸纤维素"@zh ;
    skos:related <http://rdaregistry.info/termList/RDAMaterial/1029>,
        <http://rdaregistry.info/termList/RDAMaterial/1033> .

<http://rdaregistry.info/termList/RDAMaterial/1026> a skos:Concept ;
    rdakit:toolkitDefinition "Ein Trägermaterial, das aus Kalbs-, Schafs- oder Ziegenhaut besteht, die aufbereitet wurde, um eine dünne, starke, durchscheinende oder undurchsichtige Substanz zum Schreiben, Buchbinden oder für andere Verwendungen zu erzeugen."@de,
        "A material consisting of calf, sheep, or goat skin which has been prepared to produce a thin, strong, translucent or opaque substance for writing, bookbinding, or other uses."@en,
        "Een basismateriaal bestaande uit kalfs-, schaaps- of geitenhuid die bewerkt is om een dunne, sterke, doorzichtige of ondoorzichtige substantie te verkrijgen voor schrijven, boekbinden of andere toepassingen."@nl,
        "由牛皮、绵羊皮或山羊皮制成的薄而坚固的半透明或不透明物质构成的基底材料，用于书写、装订或其他用途。"@zh ;
    rdakit:toolkitLabel "Pergament"@de,
        "parchment"@en,
        "pergamino"@es,
        "parchemin"@fr,
        "perkament"@nl,
        "pergament"@sv,
        "羊皮纸"@zh ;
    reg:identifier <http://metadataregistry.org/concepts/8480> ;
    reg:status <http://metadataregistry.org/uri/RegStatus/1001> ;
    skos:definition "Ein Trägermaterial, das aus Kalbs-, Schafs- oder Ziegenhaut besteht, die aufbereitet wurde, um eine dünne, starke, durchscheinende oder undurchsichtige Substanz zum Schreiben, Buchbinden oder für andere Verwendungen zu erzeugen."@de,
        "A material consisting of calf, sheep, or goat skin which has been prepared to produce a thin, strong, translucent or opaque substance for writing, bookbinding, or other uses."@en,
        "Een basismateriaal bestaande uit kalfs-, schaaps- of geitenhuid die bewerkt is om een dunne, sterke, doorzichtige of ondoorzichtige substantie te verkrijgen voor schrijven, boekbinden of andere toepassingen."@nl,
        "由牛皮、绵羊皮或山羊皮制成的薄而坚固的半透明或不透明物质构成的基底材料，用于书写、装订或其他用途。"@zh ;
    skos:inScheme <http://rdaregistry.info/termList/RDAMaterial> ;
    skos:prefLabel "Pergament"@de,
        "parchment"@en,
        "pergamino"@es,
        "parchemin"@fr,
        "perkament"@nl,
        "pergament"@sv,
        "羊皮纸"@zh ;
    skos:related <http://rdaregistry.info/termList/RDAMaterial/1035>,
        <http://rdaregistry.info/termList/RDAMaterial/1041> .

<http://rdaregistry.info/termList/RDAMaterial/1035> a skos:Concept ;
    rdakit:toolkitDefinition "Ein Trägermaterial, das aus der Haut von Tieren wie Schafen, Ziegen oder Kälbern besteht, die vom Körper getrennt wurde und auf verschiedene Arten bearbeitet wird, um Haare zu entfernen, zu trocknen, färben und anderweitig zurecht gemacht zu werden."@de,
        "A material consisting of the integument of animals, such as sheep, goats, or calves, separated from the body and variously processed to remove hair, dry, tan, or otherwise dress."@en,
        "Een basismateriaal bestaande uit het vel van dieren, zoals schapen, geiten of kalveren, verwijderd van het lichaam en behandeld op diverse manieren om haren te verwijderen, te drogen, te looien of anderszins opgemaakt."@nl,
        "绵羊、山羊或小牛等动物的外皮经剥皮和各种工序处理后去除毛发、晒干或硝鞣而构成的基底材料。"@zh ;
    rdakit:toolkitLabel "Fell"@de,
        "skin"@en,
        "piel"@es,
        "peau"@fr,
        "huid"@nl,
        "skinn"@sv,
        "皮"@zh ;
    reg:identifier <http://metadataregistry.org/concepts/8489> ;
    reg:status <http://metadataregistry.org/uri/RegStatus/1001> ;
    skos:definition "Ein Trägermaterial, das aus der Haut von Tieren wie Schafen, Ziegen oder Kälbern besteht, die vom Körper getrennt wurde und auf verschiedene Arten bearbeitet wird, um Haare zu entfernen, zu trocknen, färben und anderweitig zurecht gemacht zu werden."@de,
        "A material consisting of the integument of animals, such as sheep, goats, or calves, separated from the body and variously processed to remove hair, dry, tan, or otherwise dress."@en,
        "Een basismateriaal bestaande uit het vel van dieren, zoals schapen, geiten of kalveren, verwijderd van het lichaam en behandeld op diverse manieren om haren te verwijderen, te drogen, te looien of anderszins opgemaakt."@nl,
        "绵羊、山羊或小牛等动物的外皮经剥皮和各种工序处理后去除毛发、晒干或硝鞣而构成的基底材料。"@zh ;
    skos:inScheme <http://rdaregistry.info/termList/RDAMaterial> ;
    skos:prefLabel "Fell"@de,
        "skin"@en,
        "piel"@es,
        "peau"@fr,
        "huid"@nl,
        "skinn"@sv,
        "皮"@zh ;
    skos:related <http://rdaregistry.info/termList/RDAMaterial/1020>,
        <http://rdaregistry.info/termList/RDAMaterial/1026> .

<http://rdaregistry.info/termList/RDAMaterial/1010> a skos:Concept ;
    rdakit:toolkitDefinition "A material made by treating cellulose with acetic acid."@en,
        "Een basismateriaal gemaakt door cellulose te behandelen met azijnzuur."@nl,
        "经醋酸处理的纤维素制成的基底材料。"@zh ;
    rdakit:toolkitLabel "diacetate"@en,
        "diacetaat"@nl,
        "diacetat"@sv,
        "双醋酸纤维素"@zh ;
    reg:identifier <http://metadataregistry.org/concepts/8464> ;
    reg:status <http://metadataregistry.org/uri/RegStatus/1001> ;
    skos:altLabel "cellulose diacetate"@en,
        "二乙酸纤维素"@zh ;
    skos:definition "A material made by treating cellulose with acetic acid."@en,
        "Een basismateriaal gemaakt door cellulose te behandelen met azijnzuur."@nl,
        "经醋酸处理的纤维素制成的基底材料。"@zh ;
    skos:inScheme <http://rdaregistry.info/termList/RDAMaterial> ;
    skos:prefLabel "diacetate"@en,
        "diacetaat"@nl,
        "diacetat"@sv,
        "双醋酸纤维素"@zh ;
    skos:related <http://rdaregistry.info/termList/RDAMaterial/1029>,
        <http://rdaregistry.info/termList/RDAMaterial/1033>,
        <http://rdaregistry.info/termList/RDAMaterial/1040> .

<http://rdaregistry.info/termList/RDAMaterial/1030> a skos:Concept ;
    rdakit:toolkitDefinition "A material that is a category of polymers that contain the ester functional group in their main chain."@en,
        "Een basismateriaal dat een categorie van polymeren is die de functionele groep van de ester bevatten in hun hoofdverbinding."@nl,
        "基底材料为主链上包含酯基团的聚合物。"@zh ;
    rdakit:toolkitLabel "polyester"@en,
        "polyester"@nl,
        "polyester"@sv,
        "聚酯纤维素"@zh ;
    reg:identifier <http://metadataregistry.org/concepts/8484> ;
    reg:status <http://metadataregistry.org/uri/RegStatus/1001> ;
    skos:definition "A material that is a category of polymers that contain the ester functional group in their main chain."@en,
        "Een basismateriaal dat een categorie van polymeren is die de functionele groep van de ester bevatten in hun hoofdverbinding."@nl,
        "基底材料为主链上包含酯基团的聚合物。"@zh ;
    skos:inScheme <http://rdaregistry.info/termList/RDAMaterial> ;
    skos:prefLabel "polyester"@en,
        "polyester"@nl,
        "polyester"@sv,
        "聚酯纤维素"@zh ;
    skos:related <http://rdaregistry.info/termList/RDAMaterial/1029>,
        <http://rdaregistry.info/termList/RDAMaterial/1033>,
        <http://rdaregistry.info/termList/RDAMaterial/1040> .

<http://rdaregistry.info/termList/RDAMaterial/1033> a skos:Concept ;
    rdakit:toolkitDefinition "A material consisting of nonflammable cellulose acetate or polyester."@en,
        "Een basismateriaal bestaande uit niet-ontvlambare celluloseacetaat of polyester."@nl,
        "由不易燃的醋酸纤维素或聚酯纤维素构成的基底材料。"@zh ;
    rdakit:toolkitLabel "safety base"@en,
        "veilige basis"@nl,
        "säkerhetsfilm"@sv,
        "安全基底"@zh ;
    reg:identifier <http://metadataregistry.org/concepts/8487> ;
    reg:status <http://metadataregistry.org/uri/RegStatus/1001> ;
    skos:definition "A material consisting of nonflammable cellulose acetate or polyester."@en,
        "Een basismateriaal bestaande uit niet-ontvlambare celluloseacetaat of polyester."@nl,
        "由不易燃的醋酸纤维素或聚酯纤维素构成的基底材料。"@zh ;
    skos:inScheme <http://rdaregistry.info/termList/RDAMaterial> ;
    skos:prefLabel "safety base"@en,
        "veilige basis"@nl,
        "säkerhetsfilm"@sv,
        "安全基底"@zh ;
    skos:related <http://rdaregistry.info/termList/RDAMaterial/1010>,
        <http://rdaregistry.info/termList/RDAMaterial/1023>,
        <http://rdaregistry.info/termList/RDAMaterial/1030>,
        <http://rdaregistry.info/termList/RDAMaterial/1040> .

<http://rdaregistry.info/termList/RDAMaterial/1029> a skos:Concept ;
    rdakit:toolkitDefinition "Ein Trägermaterial, das aus synthetischen oder halbsynthethischen organischen Polymeren mit hohen Molekulargewicht besteht, die formbar sind."@de,
        "A material consisting of synthetic or semi-synthetic organic polymers of high molecular weight that are moldable."@en,
        "Een bevestigd materiaal of basismateriaal bestaande uit synthetische of semi-synthetische organische polymeren van een hoog moleculair gewicht die kneedbaar zijn."@nl,
        "由合成或半合成可塑高分子量有机聚合物构成的应用材料或基底材料。"@zh ;
    rdakit:toolkitLabel "Plastik"@de,
        "plastic"@en,
        "plástico"@es,
        "plastique"@fr,
        "plastic"@nl,
        "plast"@sv,
        "塑料"@zh ;
    reg:identifier <http://metadataregistry.org/concepts/8483> ;
    reg:status <http://metadataregistry.org/uri/RegStatus/1001> ;
    skos:definition "Ein Trägermaterial, das aus synthetischen oder halbsynthethischen organischen Polymeren mit hohen Molekulargewicht besteht, die formbar sind."@de,
        "A material consisting of synthetic or semi-synthetic organic polymers of high molecular weight that are moldable."@en,
        "Een bevestigd materiaal of basismateriaal bestaande uit synthetische of semi-synthetische organische polymeren van een hoog moleculair gewicht die kneedbaar zijn."@nl,
        "由合成或半合成可塑高分子量有机聚合物构成的应用材料或基底材料。"@zh ;
    skos:inScheme <http://rdaregistry.info/termList/RDAMaterial> ;
    skos:prefLabel "Plastik"@de,
        "plastic"@en,
        "plástico"@es,
        "plastique"@fr,
        "plastic"@nl,
        "plast"@sv,
        "塑料"@zh ;
    skos:related <http://rdaregistry.info/termList/RDAMaterial/1001>,
        <http://rdaregistry.info/termList/RDAMaterial/1010>,
        <http://rdaregistry.info/termList/RDAMaterial/1023>,
        <http://rdaregistry.info/termList/RDAMaterial/1030>,
        <http://rdaregistry.info/termList/RDAMaterial/1040> .

<http://rdaregistry.info/termList/RDAMaterial/1040> a skos:Concept ;
    rdakit:toolkitDefinition "A material manufactured from cellulose and a source of acetate esters, typically acetic anhydride."@en,
        "Een basismateriaal vervaardigd uit cellulose en een bron van acetaat-esters, meestal azijnzuuranhydride."@nl,
        "由纤维素和醋酸酯，特别是乙酸酐制成的基底材料。"@zh ;
    rdakit:toolkitLabel "triacetate"@en,
        "triacetaat"@nl,
        "triacetat"@sv,
        "三醋酸纤维素"@zh ;
    reg:identifier <http://metadataregistry.org/concepts/8494> ;
    reg:status <http://metadataregistry.org/uri/RegStatus/1001> ;
    skos:altLabel "cellulose triacetate"@en,
        "三乙酸纤维素"@zh ;
    skos:definition "A material manufactured from cellulose and a source of acetate esters, typically acetic anhydride."@en,
        "Een basismateriaal vervaardigd uit cellulose en een bron van acetaat-esters, meestal azijnzuuranhydride."@nl,
        "由纤维素和醋酸酯，特别是乙酸酐制成的基底材料。"@zh ;
    skos:inScheme <http://rdaregistry.info/termList/RDAMaterial> ;
    skos:prefLabel "triacetate"@en,
        "triacetaat"@nl,
        "triacetat"@sv,
        "三醋酸纤维素"@zh ;
    skos:related <http://rdaregistry.info/termList/RDAMaterial/1001>,
        <http://rdaregistry.info/termList/RDAMaterial/1010>,
        <http://rdaregistry.info/termList/RDAMaterial/1029>,
        <http://rdaregistry.info/termList/RDAMaterial/1030>,
        <http://rdaregistry.info/termList/RDAMaterial/1033> .

<http://metadataregistry.org/uri/RegStatus/1001> a skos:Concept ;
    skos:prefLabel "Published"@en .

<http://rdaregistry.info/termList/RDAMaterial> a skos:ConceptScheme ;
    dc:title "RDA Material" .

