@prefix dc: <http://purl.org/dc/elements/1.1/> .
@prefix rdakit: <http://metadataregistry.org/uri/profile/rdakit/> .
@prefix rdf: <http://www.w3.org/1999/02/22-rdf-syntax-ns#> .
@prefix rdfs: <http://www.w3.org/2000/01/rdf-schema#> .
@prefix reg: <http://metadataregistry.org/uri/profile/regap/> .
@prefix skos: <http://www.w3.org/2004/02/skos/core#> .
@prefix xml: <http://www.w3.org/XML/1998/namespace> .
@prefix xsd: <http://www.w3.org/2001/XMLSchema#> .

<http://rdaregistry.info/termList/RDARegionalEncoding/1001> a skos:Concept ;
    rdakit:toolkitDefinition "A regional encoding for a videodisc or video game carrier, permitting playback on devices worldwide."@en ;
    rdakit:toolkitLabel "all regions"@en ;
    reg:identifier <http://metadataregistry.org/concepts/9478> ;
    reg:status <http://metadataregistry.org/uri/RegStatus/1001> ;
    skos:altLabel "no regional encoding"@en,
        "region 0"@en,
        "region 9"@en,
        "region ABC"@en,
        "region free"@en ;
    skos:definition "A regional encoding for a videodisc or video game carrier, permitting playback on devices worldwide."@en ;
    skos:inScheme <http://rdaregistry.info/termList/RDARegionalEncoding> ;
    skos:prefLabel "all regions"@en .

<http://rdaregistry.info/termList/RDARegionalEncoding/1002> a skos:Concept ;
    rdakit:toolkitDefinition "A regional encoding for a DVD videodisc encoded for playback by devices configured to decode it in the United States, Canada, Bermuda, and U.S. territories."@en ;
    rdakit:toolkitLabel "region 1"@en ;
    reg:identifier <http://metadataregistry.org/concepts/9479> ;
    reg:status <http://metadataregistry.org/uri/RegStatus/1001> ;
    skos:definition "A regional encoding for a DVD videodisc encoded for playback by devices configured to decode it in the United States, Canada, Bermuda, and U.S. territories."@en ;
    skos:inScheme <http://rdaregistry.info/termList/RDARegionalEncoding> ;
    skos:prefLabel "region 1"@en .

<http://rdaregistry.info/termList/RDARegionalEncoding/1003> a skos:Concept ;
    rdakit:toolkitDefinition "A regional encoding for a Blu-ray videodisc encoded for playback by devices configured to decode it in North America, Central America, South America, Japan, North Korea, South Korea, Taiwan, Hong Kong, and Southeast Asia."@en ;
    rdakit:toolkitLabel "region A"@en ;
    reg:identifier <http://metadataregistry.org/concepts/9480> ;
    reg:status <http://metadataregistry.org/uri/RegStatus/1001> ;
    skos:definition "A regional encoding for a Blu-ray videodisc encoded for playback by devices configured to decode it in North America, Central America, South America, Japan, North Korea, South Korea, Taiwan, Hong Kong, and Southeast Asia."@en ;
    skos:inScheme <http://rdaregistry.info/termList/RDARegionalEncoding> ;
    skos:prefLabel "region A"@en .

<http://rdaregistry.info/termList/RDARegionalEncoding/1004> a skos:Concept ;
    rdakit:toolkitDefinition "A regional encoding for a DVD videodisc encoded for playback by devices configured to decode it in Japan, Europe, South Africa, and the Middle East, including Egypt."@en ;
    rdakit:toolkitLabel "region 2"@en ;
    reg:identifier <http://metadataregistry.org/concepts/9481> ;
    reg:status <http://metadataregistry.org/uri/RegStatus/1001> ;
    skos:definition "A regional encoding for a DVD videodisc encoded for playback by devices configured to decode it in Japan, Europe, South Africa, and the Middle East, including Egypt."@en ;
    skos:inScheme <http://rdaregistry.info/termList/RDARegionalEncoding> ;
    skos:prefLabel "region 2"@en .

<http://rdaregistry.info/termList/RDARegionalEncoding/1005> a skos:Concept ;
    rdakit:toolkitDefinition "A regional encoding for a Blu-ray videodisc encoded for playback by devices configured to decode it in Europe, Greenland, French territories, Middle East, Africa, Australia, and New Zealand."@en ;
    rdakit:toolkitLabel "region B"@en ;
    reg:identifier <http://metadataregistry.org/concepts/9482> ;
    reg:status <http://metadataregistry.org/uri/RegStatus/1001> ;
    skos:definition "A regional encoding for a Blu-ray videodisc encoded for playback by devices configured to decode it in Europe, Greenland, French territories, Middle East, Africa, Australia, and New Zealand."@en ;
    skos:inScheme <http://rdaregistry.info/termList/RDARegionalEncoding> ;
    skos:prefLabel "region B"@en .

<http://rdaregistry.info/termList/RDARegionalEncoding/1006> a skos:Concept ;
    rdakit:toolkitDefinition "A regional encoding for a DVD videodisc encoded for playback by devices configured to decode it in international venues such as aircraft, cruise ships, spacecraft, etc."@en ;
    rdakit:toolkitLabel "region 8"@en ;
    reg:identifier <http://metadataregistry.org/concepts/9483> ;
    reg:status <http://metadataregistry.org/uri/RegStatus/1001> ;
    skos:definition "A regional encoding for a DVD videodisc encoded for playback by devices configured to decode it in international venues such as aircraft, cruise ships, spacecraft, etc."@en ;
    skos:inScheme <http://rdaregistry.info/termList/RDARegionalEncoding> ;
    skos:prefLabel "region 8"@en .

<http://rdaregistry.info/termList/RDARegionalEncoding/1007> a skos:Concept ;
    rdakit:toolkitDefinition "A regional encoding for a DVD videodisc encoded for playback by devices configured to decode it for special uses, such as playing protected copies sent to film industry professionals or to the media."@en ;
    rdakit:toolkitLabel "region 7"@en ;
    reg:identifier <http://metadataregistry.org/concepts/9484> ;
    reg:status <http://metadataregistry.org/uri/RegStatus/1001> ;
    skos:definition "A regional encoding for a DVD videodisc encoded for playback by devices configured to decode it for special uses, such as playing protected copies sent to film industry professionals or to the media."@en ;
    skos:inScheme <http://rdaregistry.info/termList/RDARegionalEncoding> ;
    skos:prefLabel "region 7"@en .

<http://rdaregistry.info/termList/RDARegionalEncoding/1008> a skos:Concept ;
    rdakit:toolkitDefinition "A regional encoding for a DVD videodisc encoded for playback by devices configured to decode it in Southeast Asia and East Asia, including Hong Kong."@en ;
    rdakit:toolkitLabel "region 3"@en ;
    reg:identifier <http://metadataregistry.org/concepts/9485> ;
    reg:status <http://metadataregistry.org/uri/RegStatus/1001> ;
    skos:definition "A regional encoding for a DVD videodisc encoded for playback by devices configured to decode it in Southeast Asia and East Asia, including Hong Kong."@en ;
    skos:inScheme <http://rdaregistry.info/termList/RDARegionalEncoding> ;
    skos:prefLabel "region 3"@en .

<http://rdaregistry.info/termList/RDARegionalEncoding/1009> a skos:Concept ;
    rdakit:toolkitDefinition "A regional encoding for a video game encoded for playback by devices configured to decode it in China."@en ;
    rdakit:toolkitLabel "region C (video game)"@en ;
    reg:identifier <http://metadataregistry.org/concepts/9486> ;
    reg:status <http://metadataregistry.org/uri/RegStatus/1001> ;
    skos:definition "A regional encoding for a video game encoded for playback by devices configured to decode it in China."@en ;
    skos:inScheme <http://rdaregistry.info/termList/RDARegionalEncoding> ;
    skos:prefLabel "region C (video game)"@en .

<http://rdaregistry.info/termList/RDARegionalEncoding/1010> a skos:Concept ;
    rdakit:toolkitDefinition "A regional encoding for a DVD videodisc encoded for playback by devices configured to decode it in Australia, New Zealand, Pacific Islands, Central America, South America, and the Caribbean."@en ;
    rdakit:toolkitLabel "region 4"@en ;
    reg:identifier <http://metadataregistry.org/concepts/9487> ;
    reg:status <http://metadataregistry.org/uri/RegStatus/1001> ;
    skos:definition "A regional encoding for a DVD videodisc encoded for playback by devices configured to decode it in Australia, New Zealand, Pacific Islands, Central America, South America, and the Caribbean."@en ;
    skos:inScheme <http://rdaregistry.info/termList/RDARegionalEncoding> ;
    skos:prefLabel "region 4"@en .

<http://rdaregistry.info/termList/RDARegionalEncoding/1011> a skos:Concept ;
    rdakit:toolkitDefinition "A regional encoding for a DVD videodisc encoded for playback by devices configured to decode it in Eastern Europe, Baltic States, Russia, Central and South Asia, Indian subcontinent, Africa, North Korea, and Mongolia."@en ;
    rdakit:toolkitLabel "region 5"@en ;
    reg:identifier <http://metadataregistry.org/concepts/9488> ;
    reg:status <http://metadataregistry.org/uri/RegStatus/1001> ;
    skos:definition "A regional encoding for a DVD videodisc encoded for playback by devices configured to decode it in Eastern Europe, Baltic States, Russia, Central and South Asia, Indian subcontinent, Africa, North Korea, and Mongolia."@en ;
    skos:inScheme <http://rdaregistry.info/termList/RDARegionalEncoding> ;
    skos:prefLabel "region 5"@en .

<http://rdaregistry.info/termList/RDARegionalEncoding/1012> a skos:Concept ;
    rdakit:toolkitDefinition "A regional encoding for a Blu-ray videodisc encoded for playback by devices configured to decode it in India, Nepal, mainland China, Russia, Central Asia, and South Asia."@en ;
    rdakit:toolkitLabel "region C (Blu-ray)"@en ;
    reg:identifier <http://metadataregistry.org/concepts/9489> ;
    reg:status <http://metadataregistry.org/uri/RegStatus/1001> ;
    skos:definition "A regional encoding for a Blu-ray videodisc encoded for playback by devices configured to decode it in India, Nepal, mainland China, Russia, Central Asia, and South Asia."@en ;
    skos:inScheme <http://rdaregistry.info/termList/RDARegionalEncoding> ;
    skos:prefLabel "region C (Blu-ray)"@en .

<http://rdaregistry.info/termList/RDARegionalEncoding/1013> a skos:Concept ;
    rdakit:toolkitDefinition "A regional encoding for a video game carrier encoded for playback by devices configured to decode it in Japan, South Korea, Taiwan, Hong Kong, Macau, and Southeast Asia."@en ;
    rdakit:toolkitLabel "region J"@en ;
    reg:identifier <http://metadataregistry.org/concepts/9490> ;
    reg:status <http://metadataregistry.org/uri/RegStatus/1001> ;
    skos:definition "A regional encoding for a video game carrier encoded for playback by devices configured to decode it in Japan, South Korea, Taiwan, Hong Kong, Macau, and Southeast Asia."@en ;
    skos:inScheme <http://rdaregistry.info/termList/RDARegionalEncoding> ;
    skos:prefLabel "region J"@en .

<http://rdaregistry.info/termList/RDARegionalEncoding/1014> a skos:Concept ;
    rdakit:toolkitDefinition "A regional encoding for a video game carrier encoded for playback by devices configured to decode it in the United States, Canada, Mexico, and South America."@en ;
    rdakit:toolkitLabel "region U/C"@en ;
    reg:identifier <http://metadataregistry.org/concepts/9491> ;
    reg:status <http://metadataregistry.org/uri/RegStatus/1001> ;
    skos:definition "A regional encoding for a video game carrier encoded for playback by devices configured to decode it in the United States, Canada, Mexico, and South America."@en ;
    skos:inScheme <http://rdaregistry.info/termList/RDARegionalEncoding> ;
    skos:prefLabel "region U/C"@en .

<http://rdaregistry.info/termList/RDARegionalEncoding/1015> a skos:Concept ;
    rdakit:toolkitDefinition "A regional encoding for a DVD videodisc encoded for playback by devices configured to decode it in China."@en ;
    rdakit:toolkitLabel "region 6"@en ;
    reg:identifier <http://metadataregistry.org/concepts/9492> ;
    reg:status <http://metadataregistry.org/uri/RegStatus/1001> ;
    skos:definition "A regional encoding for a DVD videodisc encoded for playback by devices configured to decode it in China."@en ;
    skos:inScheme <http://rdaregistry.info/termList/RDARegionalEncoding> ;
    skos:prefLabel "region 6"@en .

<http://metadataregistry.org/uri/RegStatus/1001> a skos:Concept ;
    skos:prefLabel "Published"@en .

<http://rdaregistry.info/termList/RDARegionalEncoding> a skos:ConceptScheme ;
    dc:title "RDA Regional Encoding" .

