@prefix dc: <http://purl.org/dc/elements/1.1/> .
@prefix rdakit: <http://metadataregistry.org/uri/profile/rdakit/> .
@prefix rdf: <http://www.w3.org/1999/02/22-rdf-syntax-ns#> .
@prefix rdfs: <http://www.w3.org/2000/01/rdf-schema#> .
@prefix reg: <http://metadataregistry.org/uri/profile/regap/> .
@prefix skos: <http://www.w3.org/2004/02/skos/core#> .
@prefix xml: <http://www.w3.org/XML/1998/namespace> .
@prefix xsd: <http://www.w3.org/2001/XMLSchema#> .

<http://rdaregistry.info/termList/specPlayback/1001> a skos:Concept ;
    rdakit:toolkitDefinition "A special playback characteristic of sound that is a standard originally issued in 1982 by the CCIR for encoding interlaced analog video signals in digital video form."@en ;
    rdakit:toolkitLabel "CCIR encoded"@en ;
    reg:identifier <http://metadataregistry.org/concepts/878> ;
    reg:status <http://metadataregistry.org/uri/RegStatus/1001> ;
    skos:definition "A special playback characteristic of sound that is a standard originally issued in 1982 by the CCIR for encoding interlaced analog video signals in digital video form."@en ;
    skos:inScheme <http://rdaregistry.info/termList/specPlayback> ;
    skos:prefLabel "CCIR encoded"@en .

<http://rdaregistry.info/termList/specPlayback/1002> a skos:Concept ;
    rdakit:toolkitDefinition "A special playback characteristic of sound that is a noise reduction system for recorded analog audio developed by CBS Laboratories in the late 1970s."@en ;
    rdakit:toolkitLabel "CX encoded"@en ;
    reg:identifier <http://metadataregistry.org/concepts/879> ;
    reg:status <http://metadataregistry.org/uri/RegStatus/1001> ;
    skos:definition "A special playback characteristic of sound that is a noise reduction system for recorded analog audio developed by CBS Laboratories in the late 1970s."@en ;
    skos:inScheme <http://rdaregistry.info/termList/specPlayback> ;
    skos:prefLabel "CX encoded"@en .

<http://rdaregistry.info/termList/specPlayback/1003> a skos:Concept ;
    rdakit:toolkitDefinition "A special playback characteristic of sound that is a family of noise reduction systems developed by dbx."@en ;
    rdakit:toolkitLabel "dbx encoded"@en ;
    reg:identifier <http://metadataregistry.org/concepts/880> ;
    reg:status <http://metadataregistry.org/uri/RegStatus/1001> ;
    skos:definition "A special playback characteristic of sound that is a family of noise reduction systems developed by dbx."@en ;
    skos:inScheme <http://rdaregistry.info/termList/specPlayback> ;
    skos:prefLabel "dbx encoded"@en .

<http://rdaregistry.info/termList/specPlayback/1004> a skos:Concept ;
    rdakit:toolkitDefinition "A special playback characteristic of sound that is a series of noise reduction systems developed by Dolby Laboratories for use in analog magnetic tape recording."@en ;
    rdakit:toolkitLabel "Dolby"@en ;
    reg:identifier <http://metadataregistry.org/concepts/881> ;
    reg:status <http://metadataregistry.org/uri/RegStatus/1001> ;
    skos:definition "A special playback characteristic of sound that is a series of noise reduction systems developed by Dolby Laboratories for use in analog magnetic tape recording."@en ;
    skos:inScheme <http://rdaregistry.info/termList/specPlayback> ;
    skos:prefLabel "Dolby"@en .

<http://rdaregistry.info/termList/specPlayback/1005> a skos:Concept ;
    rdakit:toolkitDefinition "A special playback characteristic of sound that is a noise reduction system developed by Dolby Laboratories for professional use in analog magnetic tape recording."@en ;
    rdakit:toolkitLabel "Dolby-A encoded"@en ;
    reg:identifier <http://metadataregistry.org/concepts/882> ;
    reg:status <http://metadataregistry.org/uri/RegStatus/1001> ;
    skos:definition "A special playback characteristic of sound that is a noise reduction system developed by Dolby Laboratories for professional use in analog magnetic tape recording."@en ;
    skos:inScheme <http://rdaregistry.info/termList/specPlayback> ;
    skos:prefLabel "Dolby-A encoded"@en .

<http://rdaregistry.info/termList/specPlayback/1006> a skos:Concept ;
    rdakit:toolkitDefinition "A special playback characteristic of sound that is a noise reduction system developed by Dolby Laboratories as a simplified version of Dolby-A for consumer use in analog magnetic tape recording."@en ;
    rdakit:toolkitLabel "Dolby-B encoded"@en ;
    reg:identifier <http://metadataregistry.org/concepts/883> ;
    reg:status <http://metadataregistry.org/uri/RegStatus/1001> ;
    skos:definition "A special playback characteristic of sound that is a noise reduction system developed by Dolby Laboratories as a simplified version of Dolby-A for consumer use in analog magnetic tape recording."@en ;
    skos:inScheme <http://rdaregistry.info/termList/specPlayback> ;
    skos:prefLabel "Dolby-B encoded"@en .

<http://rdaregistry.info/termList/specPlayback/1007> a skos:Concept ;
    rdakit:toolkitDefinition "A special playback characteristic of sound that is a noise reduction system developed by Dolby Laboratories in 1980 as a combined version of Dolby-A and Dolby-B for use in analog magnetic tape recording."@en ;
    rdakit:toolkitLabel "Dolby-C encoded"@en ;
    reg:identifier <http://metadataregistry.org/concepts/884> ;
    reg:status <http://metadataregistry.org/uri/RegStatus/1001> ;
    skos:definition "A special playback characteristic of sound that is a noise reduction system developed by Dolby Laboratories in 1980 as a combined version of Dolby-A and Dolby-B for use in analog magnetic tape recording."@en ;
    skos:inScheme <http://rdaregistry.info/termList/specPlayback> ;
    skos:prefLabel "Dolby-C encoded"@en .

<http://rdaregistry.info/termList/specPlayback/1008> a skos:Concept ;
    rdakit:toolkitDefinition "A special playback characteristic of sound that is a digital sampling of analogue sound based on the pulse-code modulation method."@en ;
    rdakit:toolkitLabel "LPCM"@en ;
    reg:identifier <http://metadataregistry.org/concepts/885> ;
    reg:status <http://metadataregistry.org/uri/RegStatus/1001> ;
    skos:altLabel "Linear pulse-code modulation"@en ;
    skos:definition "A special playback characteristic of sound that is a digital sampling of analogue sound based on the pulse-code modulation method."@en ;
    skos:inScheme <http://rdaregistry.info/termList/specPlayback> ;
    skos:prefLabel "LPCM"@en .

<http://rdaregistry.info/termList/specPlayback/1009> a skos:Concept ;
    rdakit:toolkitDefinition "A special playback characteristic of sound that follows the standards of the National Association of Broadcasters."@en ;
    rdakit:toolkitLabel "NAB standard"@en ;
    reg:identifier <http://metadataregistry.org/concepts/886> ;
    reg:status <http://metadataregistry.org/uri/RegStatus/1001> ;
    skos:definition "A special playback characteristic of sound that follows the standards of the National Association of Broadcasters."@en ;
    skos:inScheme <http://rdaregistry.info/termList/specPlayback> ;
    skos:prefLabel "NAB standard"@en .

<http://metadataregistry.org/uri/RegStatus/1001> a skos:Concept ;
    skos:prefLabel "Published"@en .

<http://rdaregistry.info/termList/specPlayback> a skos:ConceptScheme ;
    dc:title "RDA Special Playback Characteristic" .

