@prefix dc: <http://purl.org/dc/elements/1.1/> .
@prefix foaf: <http://xmlns.com/foaf/0.1/> .
@prefix rdakit: <http://metadataregistry.org/uri/profile/rdakit/> .
@prefix rdf: <http://www.w3.org/1999/02/22-rdf-syntax-ns#> .
@prefix rdfs: <http://www.w3.org/2000/01/rdf-schema#> .
@prefix reg: <http://metadataregistry.org/uri/profile/regap/> .
@prefix skos: <http://www.w3.org/2004/02/skos/core#> .
@prefix xml: <http://www.w3.org/XML/1998/namespace> .
@prefix xsd: <http://www.w3.org/2001/XMLSchema#> .

<http://rdaregistry.info/Elements/m/P30001> a rdf:Property ;
    rdfs:label "has carrier type"@en,
        "a pour type de support matériel"@fr,
        "har bärartyp"@sv ;
    rdakit:instructionNumber "3.3" ;
    rdakit:toolkitDefinition "A categorization reflecting the format of the storage medium and housing of a carrier in combination with the type of intermediation device required to view, play, run, etc., the content of a manifestation."@en,
        "Una categorización que refleja el formato del medio de almacenamiento y alojamiento de un soporte en combinación con el tipo de aparato de intermediación requerido para ver, reproducir, operar, etc., el contenido de un recurso."@es,
        "Catégorisation reflétant le format du support de stockage et du contenant d’un support matériel combiné avec le type de dispositif de médiation requis pour visionner, faire fonctionner, faire défiler, etc. le contenu d’une ressource."@fr ;
    rdakit:toolkitLabel "carrier type"@en,
        "tipo de soporte"@es,
        "type de support matériel"@fr,
        "bärartyp"@sv ;
    reg:hasUnconstrained <http://rdaregistry.info/Elements/u/P60048> ;
    reg:lexicalAlias <http://rdaregistry.info/Elements/m/carrierType.en> ;
    reg:name "carrierType"@en ;
    reg:status <http://metadataregistry.org/uri/RegStatus/1001> ;
    rdfs:domain <http://rdaregistry.info/Elements/c/C10007> ;
    rdfs:isDefinedBy <http://rdaregistry.info/Elements/m/> ;
    skos:definition "Relates a manifestation to a categorization reflecting the format of the storage medium and housing of a carrier in combination with the type of intermediation device required to view, play, run, etc., the content of a manifestation."@en,
        "Met une manifestation en relation avec une catégorisation reflétant le format du support de stockage et du contenant d’un support matériel combiné avec le type de dispositif de médiation requis pour visionner, faire fonctionner, faire défiler, etc. le contenu d’une ressource."@fr .

<http://rdaregistry.info/Elements/m/P30002> a rdf:Property ;
    rdfs:label "has media type"@en,
        "a pour type de média"@fr,
        "har medietyp"@sv ;
    rdakit:instructionNumber "3.2" ;
    rdakit:toolkitDefinition "A categorization reflecting the general type of intermediation device required to view, play, run, etc., the content of a manifestation."@en,
        "Una categorización que refleja el tipo general de elemento de intermediación que se requiere para ver, reproducir, operar, etc., el contenido de un recurso."@es,
        "Catégorisation indiquant le type général de dispositif de médiation requis pour visionner, faire fonctionner, faire défiler, etc. le contenu d’une ressource."@fr ;
    rdakit:toolkitLabel "media type"@en,
        "tipo de medio"@es,
        "type de média"@fr,
        "medietyp"@sv ;
    reg:hasUnconstrained <http://rdaregistry.info/Elements/u/P60050> ;
    reg:lexicalAlias <http://rdaregistry.info/Elements/m/mediaType.en> ;
    reg:name "mediaType"@en ;
    reg:status <http://metadataregistry.org/uri/RegStatus/1001> ;
    rdfs:domain <http://rdaregistry.info/Elements/c/C10007> ;
    rdfs:isDefinedBy <http://rdaregistry.info/Elements/m/> ;
    skos:definition "Relates a manifestation to a categorization reflecting the general type of intermediation device required to view, play, run, etc., the content of a manifestation."@en,
        "Met une manifestation en relation avec une catégorisation indiquant le type général de dispositif de médiation requis pour visionner, faire fonctionner, faire défiler, etc. le contenu d’une ressource."@fr .

<http://rdaregistry.info/Elements/m/P30003> a rdf:Property ;
    rdfs:label "has mode of issuance"@en,
        "a pour mode de parution"@fr,
        "har utgivningssätt"@sv ;
    rdakit:instructionNumber "2.13" ;
    rdakit:toolkitDefinition "A categorization reflecting whether a manifestation is issued in one or more parts, the way it is updated, and whether its termination is predetermined or not."@en,
        "Una categorización que refleja si un recurso está publicado en una o más partes, su forma de actualización y su terminación esperada."@es,
        "Catégorisation permettant de signaler si une ressource est publiée en une ou plusieurs parties, son mode de mise à jour et sa complétude visée."@fr ;
    rdakit:toolkitLabel "mode of issuance"@en,
        "modo de edición"@es,
        "mode de parution"@fr,
        "utgivningssätt"@sv ;
    reg:hasUnconstrained <http://rdaregistry.info/Elements/u/P60051> ;
    reg:lexicalAlias <http://rdaregistry.info/Elements/m/modeOfIssuance.en> ;
    reg:name "modeOfIssuance"@en ;
    reg:status <http://metadataregistry.org/uri/RegStatus/1001> ;
    rdfs:domain <http://rdaregistry.info/Elements/c/C10007> ;
    rdfs:isDefinedBy <http://rdaregistry.info/Elements/m/> ;
    skos:definition "Relates a manifestation to a categorization reflecting whether a manifestation is issued in one or more parts, the way it is updated, and whether its termination is predetermined or not."@en,
        "Met une manifestation en relation avec une catégorisation permettant de signaler si une ressource est publiée en une ou plusieurs parties, son mode de mise à jour et sa complétude visée."@fr .

<http://rdaregistry.info/Elements/m/P30005> a rdf:Property ;
    rdfs:label "has preferred citation"@en,
        "a pour citation privilégiée"@fr,
        "har föredragen referensform"@sv ;
    rdakit:instructionNumber "2.16" ;
    rdakit:toolkitDefinition "A citation for a manifestation in the form preferred by a creator, publisher, custodian, indexing or abstracting service, etc."@en,
        "Una cita de un recurso en la forma preferida por el creador, editor, custodio, servicio de indización y resúmenes, etc."@es,
        "Citation d’une ressource sous la forme privilégiée par un créateur, un éditeur, un dépositaire, un service d’indexation ou d’analyse, etc."@fr ;
    rdakit:toolkitLabel "preferred citation"@en,
        "cita preferida"@es,
        "citation privilégiée"@fr,
        "föredragen referensform"@sv ;
    reg:hasUnconstrained <http://rdaregistry.info/Elements/u/P60057> ;
    reg:lexicalAlias <http://rdaregistry.info/Elements/m/preferredCitation.en> ;
    reg:name "preferredCitation"@en ;
    reg:status <http://metadataregistry.org/uri/RegStatus/1001> ;
    rdfs:domain <http://rdaregistry.info/Elements/c/C10007> ;
    rdfs:isDefinedBy <http://rdaregistry.info/Elements/m/> ;
    skos:definition "Relates a manifestation to a citation for a manifestation in the form preferred by a creator, publisher, custodian, indexing or abstracting service, etc."@en,
        "Met une manifestation en relation avec une citation d’une ressource sous la forme privilégiée par un créateur, un éditeur, un dépositaire, un service d’indexation ou d’analyse, etc."@fr .

<http://rdaregistry.info/Elements/m/P30007> a rdf:Property ;
    rdfs:label "has copyright date"@en,
        "a pour date de copyright"@fr,
        "har copyrightår"@sv ;
    rdakit:instructionNumber "2.11" ;
    rdakit:toolkitDefinition "A date associated with a claim of protection under copyright or a similar regime."@en,
        "Una fecha asociada con el reclamo de protección bajo el régimen de derechos de autor o régimen similares."@es,
        "Date associée à une revendication de protection en vertu du copyright ou d’un régime similaire."@fr ;
    rdakit:toolkitLabel "copyright date"@en,
        "fecha de derechos de autor"@es,
        "date de copyright"@fr,
        "copyrightår"@sv ;
    reg:hasUnconstrained <http://rdaregistry.info/Elements/u/P60069> ;
    reg:lexicalAlias <http://rdaregistry.info/Elements/m/copyrightDate.en> ;
    reg:name "copyrightDate"@en ;
    reg:status <http://metadataregistry.org/uri/RegStatus/1001> ;
    rdfs:domain <http://rdaregistry.info/Elements/c/C10007> ;
    rdfs:isDefinedBy <http://rdaregistry.info/Elements/m/> ;
    skos:definition "Relates a manifestation to a date associated with a claim of protection under copyright or a similar regime."@en,
        "Met une manifestation en relation avec une date associée à une revendication de protection en vertu du copyright ou d’un régime similaire."@fr ;
    skos:scopeNote "Copyright dates include phonogram dates, that is, dates associated with claims of protection for audio recordings."@en,
        "Les dates de copyright comprennent les dates de phonogramme (c’est-à-dire les dates associées à des revendications de protection pour les enregistrements sonores, aussi appelées dates de protection)."@fr .

<http://rdaregistry.info/Elements/m/P30008> a rdf:Property ;
    rdfs:label "has date of distribution"@en,
        "a pour date de diffusion ou de distribution"@fr,
        "har distributionstid"@sv ;
    rdakit:instructionNumber "2.9.6" ;
    rdakit:toolkitDefinition "A date associated with the distribution of a manifestation in a published form."@en,
        "Una fecha asociada con la distribución de un recurso publicado."@es,
        "Date associée à la diffusion ou à la distribution d’une ressource sous une forme publiée."@fr ;
    rdakit:toolkitLabel "date of distribution"@en,
        "fecha de distribución"@es,
        "date de diffusion ou de distribution"@fr,
        "distributionstid"@sv ;
    reg:hasUnconstrained <http://rdaregistry.info/Elements/u/P60070> ;
    reg:lexicalAlias <http://rdaregistry.info/Elements/m/dateOfDistribution.en> ;
    reg:name "dateOfDistribution"@en ;
    reg:status <http://metadataregistry.org/uri/RegStatus/1001> ;
    rdfs:domain <http://rdaregistry.info/Elements/c/C10007> ;
    rdfs:isDefinedBy <http://rdaregistry.info/Elements/m/> ;
    skos:definition "Relates a manifestation to a date associated with the distribution of a manifestation in a published form."@en,
        "Met une manifestation en relation avec une date associée à la diffusion ou à la distribution d’une ressource sous une forme publiée."@fr .

<http://rdaregistry.info/Elements/m/P30009> a rdf:Property ;
    rdfs:label "has date of production"@en,
        "a pour date de production"@fr,
        "har produktionstid"@sv ;
    rdakit:instructionNumber "2.7.6" ;
    rdakit:toolkitDefinition "A date associated with the inscription, fabrication, construction, etc., of a manifestation in an unpublished form."@en,
        "Una fecha asociada con la inscripción, fabricación, construcción, etc., de un recurso producido en forma inédita."@es,
        "Date associée à la scription, la fabrication, la construction, etc. d’une ressource sous une forme non publiée."@fr ;
    rdakit:toolkitLabel "date of production"@en,
        "fecha de producción"@es,
        "date de production"@fr,
        "produktionstid"@sv ;
    reg:hasUnconstrained <http://rdaregistry.info/Elements/u/P60071> ;
    reg:lexicalAlias <http://rdaregistry.info/Elements/m/dateOfProduction.en> ;
    reg:name "dateOfProduction"@en ;
    reg:status <http://metadataregistry.org/uri/RegStatus/1001> ;
    rdfs:domain <http://rdaregistry.info/Elements/c/C10007> ;
    rdfs:isDefinedBy <http://rdaregistry.info/Elements/m/> ;
    skos:definition "Relates a manifestation to a date associated with the inscription, fabrication, construction, etc., of a manifestation in an unpublished form."@en,
        "Met une manifestation en relation avec une date associée à la scription, la fabrication, la construction, etc. d’une ressource sous une forme non publiée."@fr .

<http://rdaregistry.info/Elements/m/P30010> a rdf:Property ;
    rdfs:label "has date of manufacture"@en,
        "a pour date de fabrication"@fr,
        "har tillverkningstid"@sv ;
    rdakit:instructionNumber "2.10.6" ;
    rdakit:toolkitDefinition "A date associated with the printing, duplicating, casting, etc., of a manifestation in a published form."@en,
        "Una fecha asociada con la impresión, duplicación, armado, etc., de un recurso publicado."@es,
        "Date associée à l’impression, à la reproduction, au moulage, etc. d’une ressource sous une forme publiée."@fr ;
    rdakit:toolkitLabel "date of manufacture"@en,
        "fecha de fabricación"@es,
        "date de fabrication"@fr,
        "tillverkningstid"@sv ;
    reg:hasUnconstrained <http://rdaregistry.info/Elements/u/P60072> ;
    reg:lexicalAlias <http://rdaregistry.info/Elements/m/dateOfManufacture.en> ;
    reg:name "dateOfManufacture"@en ;
    reg:status <http://metadataregistry.org/uri/RegStatus/1001> ;
    rdfs:domain <http://rdaregistry.info/Elements/c/C10007> ;
    rdfs:isDefinedBy <http://rdaregistry.info/Elements/m/> ;
    skos:definition "Relates a manifestation to a date associated with the printing, duplicating, casting, etc., of a manifestation in a published form."@en,
        "Met une manifestation en relation avec une date associée à l’impression, à la reproduction, au moulage, etc. d’une ressource sous une forme publiée."@fr .

<http://rdaregistry.info/Elements/m/P30011> a rdf:Property ;
    rdfs:label "has date of publication"@en,
        "a pour date de publication"@fr,
        "har utgivningstid"@sv ;
    rdakit:instructionNumber "2.8.6" ;
    rdakit:toolkitDefinition "A date associated with the publication, release, or issuing of a manifestation."@en,
        "Una fecha asociada con la publicación, entrega o emisión de un recurso."@es,
        "Date associée à la publication, la mise à disposition ou l’édition d’une ressource."@fr ;
    rdakit:toolkitLabel "date of publication"@en,
        "fecha de publicación"@es,
        "date de publication"@fr,
        "utgivningstid"@sv ;
    reg:hasUnconstrained <http://rdaregistry.info/Elements/u/P60073> ;
    reg:lexicalAlias <http://rdaregistry.info/Elements/m/dateOfPublication.en> ;
    reg:name "dateOfPublication"@en ;
    reg:status <http://metadataregistry.org/uri/RegStatus/1001> ;
    rdfs:domain <http://rdaregistry.info/Elements/c/C10007> ;
    rdfs:isDefinedBy <http://rdaregistry.info/Elements/m/> ;
    skos:definition "Relates a manifestation to a date associated with the publication, release, or issuing of a manifestation."@en,
        "Met une manifestation en relation avec une date associée à la publication, la mise à disposition ou l’édition d’une ressource."@fr .

<http://rdaregistry.info/Elements/m/P30012> a rdf:Property ;
    rdfs:label "has parallel designation of named revision of edition"@en,
        "a pour indication parallèle d’une révision nommée d’une édition"@fr,
        "har parallell påföljande upplageförteckning"@sv ;
    rdakit:instructionNumber "2.5.7" ;
    rdakit:toolkitDefinition "A designation of a named revision of an edition in a language or script that differs from that recorded in a designation of a named revision of an edition element."@en,
        "Una designación de una revisión dada de una edición en una lengua y/o escritura que difiere de la registrada en el elemento designación de una revisión mencionada de una edición"@es,
        "Indication d’une révision nommée d’une édition dans une langue et/ou une écriture différentes de celles enregistrées dans l’élément Indication d’une révision nommée d’une édition."@fr ;
    rdakit:toolkitLabel "parallel designation of named revision of edition"@en,
        "designación paralela de una revisión mencionada de una edición"@es,
        "indication parallèle d’une révision nommée d’une édition"@fr,
        "parallell påföljande upplageförteckning"@sv ;
    reg:hasUnconstrained <http://rdaregistry.info/Elements/u/P60077> ;
    reg:lexicalAlias <http://rdaregistry.info/Elements/m/parallelDesignationOfNamedRevisionOfEdition.en> ;
    reg:name "parallelDesignationOfNamedRevisionOfEdition"@en ;
    reg:status <http://metadataregistry.org/uri/RegStatus/1001> ;
    rdfs:domain <http://rdaregistry.info/Elements/c/C10007> ;
    rdfs:isDefinedBy <http://rdaregistry.info/Elements/m/> ;
    skos:definition "Relates a manifestation to a designation of a named revision of an edition in a language or script that differs from that recorded in a designation of a named revision of an edition element."@en,
        "Met une manifestation en relation avec une indication d’une révision nommée d’une édition dans une langue et/ou une écriture différentes de celles enregistrées dans l’élément Indication d’une révision nommée d’une édition."@fr .

<http://rdaregistry.info/Elements/m/P30013> a rdf:Property ;
    rdfs:label "has parallel designation of edition"@en,
        "a pour indication parallèle de l’édition"@fr,
        "har parallell upplageförteckning"@sv ;
    rdakit:instructionNumber "2.5.3" ;
    rdakit:toolkitDefinition "A designation of edition in a language or script that differs from that recorded in a designation of edition element."@en,
        "Una designación de edición en una lengua y/o escritura que difiere de la registrada en el elemento designación de edición."@es,
        "Indication d’édition dans une langue et/ou une écriture différentes de celles enregistrées dans l’élément Indication de l’édition"@fr ;
    rdakit:toolkitLabel "parallel designation of edition"@en,
        "designación paralela de edición"@es,
        "indication parallèle de l’édition"@fr,
        "parallell upplageförteckning"@sv ;
    reg:hasUnconstrained <http://rdaregistry.info/Elements/u/P60078> ;
    reg:lexicalAlias <http://rdaregistry.info/Elements/m/parallelDesignationOfEdition.en> ;
    reg:name "parallelDesignationOfEdition"@en ;
    reg:status <http://metadataregistry.org/uri/RegStatus/1001> ;
    rdfs:domain <http://rdaregistry.info/Elements/c/C10007> ;
    rdfs:isDefinedBy <http://rdaregistry.info/Elements/m/> ;
    skos:definition "Relates a manifestation to a designation of edition in a language or script that differs from that recorded in a designation of edition element."@en,
        "Met une manifestation en relation avec une indication d’édition dans une langue et/ou une écriture différentes de celles enregistrées dans l’élément Indication de l’édition"@fr .

<http://rdaregistry.info/Elements/m/P30014> a rdf:Property ;
    rdfs:label "has numbering within series"@en,
        "a pour numérotation au sein de la collection"@fr,
        "har numrering inom serie"@sv ;
    rdakit:instructionNumber "2.12.9" ;
    rdakit:toolkitDefinition "A designation of the sequencing of a part or parts within a series."@en,
        "Una designación de la secuencia de una parte o partes dentro de la serie."@es,
        "Indication d’ordre séquentiel d’une ou de plusieurs parties à l’intérieur d’une collection."@fr ;
    rdakit:toolkitLabel "numbering within series"@en,
        "numeración dentro de la serie"@es,
        "numérotation au sein de la collection"@fr,
        "numrering inom serie"@sv ;
    reg:hasUnconstrained <http://rdaregistry.info/Elements/u/P60081> ;
    reg:lexicalAlias <http://rdaregistry.info/Elements/m/numberingWithinSeries.en> ;
    reg:name "numberingWithinSeries"@en ;
    reg:status <http://metadataregistry.org/uri/RegStatus/1001> ;
    rdfs:domain <http://rdaregistry.info/Elements/c/C10007> ;
    rdfs:isDefinedBy <http://rdaregistry.info/Elements/m/> ;
    skos:definition "Relates a manifestation to a designation of the sequencing of a part or parts within a series."@en,
        "Met une manifestation en relation avec une indication d’ordre séquentiel d’une ou de plusieurs parties à l’intérieur d’une collection."@fr ;
    skos:scopeNote "Numbering includes a numeral, a letter, any other character, or the combination of these with or without an accompanying caption and/or a chronological designation."@en,
        "La numérotation au sein d’une collection peut comprendre un chiffre, une lettre, tout autre caractère ou la combinaison de ces éléments, accompagnés ou non d’une appellation (volume, numéro, etc.) et/ou d’une indication chronologique."@fr .

<http://rdaregistry.info/Elements/m/P30015> a rdf:Property ;
    rdfs:label "has numbering within subseries"@en,
        "a pour numérotation au sein de la sous-collection"@fr,
        "har numrering inom underserie"@sv ;
    rdakit:instructionNumber "2.12.17" ;
    rdakit:toolkitDefinition "A designation of the sequencing of a part or parts within a subseries."@en,
        "Una designación de la secuencia de una parte o partes dentro de la subserie."@es,
        "Indication d’ordre séquentiel d’une ou de plusieurs parties à l’intérieur d’une sous-collection."@fr ;
    rdakit:toolkitLabel "numbering within subseries"@en,
        "numeración dentro de la subserie"@es,
        "numérotation au sein de la sous-collection"@fr,
        "numrering inom underserie"@sv ;
    reg:hasUnconstrained <http://rdaregistry.info/Elements/u/P60082> ;
    reg:lexicalAlias <http://rdaregistry.info/Elements/m/numberingWithinSubseries.en> ;
    reg:name "numberingWithinSubseries"@en ;
    reg:status <http://metadataregistry.org/uri/RegStatus/1001> ;
    rdfs:domain <http://rdaregistry.info/Elements/c/C10007> ;
    rdfs:isDefinedBy <http://rdaregistry.info/Elements/m/> ;
    skos:definition "Relates a manifestation to a designation of the sequencing of a part or parts within a subseries."@en,
        "Met une manifestation en relation avec une indication d’ordre séquentiel d’une ou de plusieurs parties à l’intérieur d’une sous-collection."@fr ;
    skos:scopeNote "Numbering includes a numeral, a letter, any other character, or the combination of these with or without an accompanying caption and/or a chronological designation."@en,
        "La numérotation au sein de la sous-collection peut comprendre un chiffre, une lettre, tout autre caractère ou la combinaison de ces éléments, accompagnés ou non d’une appellation (volume, numéro, etc.) et/ou d’une indication chronologique."@fr .

<http://rdaregistry.info/Elements/m/P30017> a rdf:Property ;
    rdfs:label "has parallel distributor’s name"@en,
        "a pour forme parallèle du nom du diffuseur ou du distributeur"@fr,
        "har parallellt distributörsnamn"@sv ;
    rdakit:instructionNumber "2.9.5" ;
    rdakit:toolkitDefinition "A distributor's name in a language or script that differs from that recorded in the distributor's name element."@en,
        "Un nombre de distribuidor en una lengua o escritura que difiere de la registrada en el elemento nombre del distribuidor."@es,
        "Nom de diffuseur ou de distributeur dans une langue et/ou une écriture différentes de celles enregistrées dans l’élément Nom de diffuseur ou de distributeur."@fr ;
    rdakit:toolkitLabel "parallel distributor's name"@en,
        "nombre paralelo del distribuidor"@es,
        "forme parallèle du nom du diffuseur ou du distributeur"@fr,
        "parallellt distributörsnamn"@sv ;
    reg:hasUnconstrained <http://rdaregistry.info/Elements/u/P60087> ;
    reg:lexicalAlias <http://rdaregistry.info/Elements/m/parallelDistributorsName.en> ;
    reg:name "parallelDistributorsName"@en ;
    reg:status <http://metadataregistry.org/uri/RegStatus/1001> ;
    rdfs:domain <http://rdaregistry.info/Elements/c/C10007> ;
    rdfs:isDefinedBy <http://rdaregistry.info/Elements/m/> ;
    skos:definition "Relates a manifestation to a distributor's name in a language or script that differs from that recorded in a distributor's name element."@en,
        "Met une manifestation en relation avec un nom de diffuseur ou de distributeur dans une langue et/ou une écriture différentes de celles enregistrées dans l’élément Nom de diffuseur ou de distributeur."@fr .

<http://rdaregistry.info/Elements/m/P30023> a rdf:Property ;
    reg:status <http://metadataregistry.org/uri/RegStatus/1008> ;
    rdfs:isDefinedBy <http://rdaregistry.info/Elements/m/> .

<http://rdaregistry.info/Elements/m/P30032> a rdf:Property ;
    reg:status <http://metadataregistry.org/uri/RegStatus/1008> ;
    rdfs:isDefinedBy <http://rdaregistry.info/Elements/m/> .

<http://rdaregistry.info/Elements/m/P30034> a rdf:Property ;
    reg:status <http://metadataregistry.org/uri/RegStatus/1008> ;
    rdfs:isDefinedBy <http://rdaregistry.info/Elements/m/> .

<http://rdaregistry.info/Elements/m/P30041> a rdf:Property ;
    reg:status <http://metadataregistry.org/uri/RegStatus/1008> ;
    rdfs:isDefinedBy <http://rdaregistry.info/Elements/m/> .

<http://rdaregistry.info/Elements/m/P30042> a rdf:Property ;
    reg:status <http://metadataregistry.org/uri/RegStatus/1008> ;
    rdfs:isDefinedBy <http://rdaregistry.info/Elements/m/> .

<http://rdaregistry.info/Elements/m/P30044> a rdf:Property ;
    reg:status <http://metadataregistry.org/uri/RegStatus/1008> ;
    rdfs:isDefinedBy <http://rdaregistry.info/Elements/m/> .

<http://rdaregistry.info/Elements/m/P30049> a rdf:Property ;
    rdfs:label "has parallel manufacturer’s name"@en,
        "a pour forme parallèle du nom du fabricant"@fr,
        "har parallellt tillverkningsnamn"@sv ;
    rdakit:instructionNumber "2.10.5" ;
    rdakit:toolkitDefinition "A manufacturer's name in a language or script that differs from that recorded in a manufacturer's name element."@en,
        "Un nombre del fabricante en una lengua y/o escritura que difiere de la registrada en el elemento nombre del fabricante."@es,
        "Nom de fabricant dans une langue et/ou une écriture différentes de celles enregistrées dans l’élément Nom de fabricant."@fr ;
    rdakit:toolkitLabel "parallel manufacturer's name"@en,
        "nombre paralelo del fabricante"@es,
        "forme parallèle du nom du fabricant"@fr,
        "parallellt tillverkningsnamn"@sv ;
    reg:hasUnconstrained <http://rdaregistry.info/Elements/u/P60108> ;
    reg:lexicalAlias <http://rdaregistry.info/Elements/m/parallelManufacturersName.en> ;
    reg:name "parallelManufacturersName"@en ;
    reg:status <http://metadataregistry.org/uri/RegStatus/1001> ;
    rdfs:domain <http://rdaregistry.info/Elements/c/C10007> ;
    rdfs:isDefinedBy <http://rdaregistry.info/Elements/m/> ;
    skos:definition "Relates a manifestation to a manufacturer's name in a language or script that differs from that recorded in a manufacturer's name element."@en,
        "Met une manifestation en relation avec un nom de fabricant dans une langue et/ou une écriture différentes de celles enregistrées dans l’élément Nom de fabricant."@fr .

<http://rdaregistry.info/Elements/m/P30079> a rdf:Property ;
    rdfs:label "has other agent associated with manifestation"@en,
        "a pour autre personne, famille ou collectivité associée à une manifestation"@fr,
        "har övrig person, familj/släkt eller institution knuten till en manifestation"@sv ;
    rdakit:instructionNumber "21.6" ;
    rdakit:toolkitDefinition "An agent other than a producer, publisher, distributor, or manufacturer associated with a manifestation."@en,
        "Una persona, familia o entidad corporativa diferente a un productor, editor, distribuidor o fabricante que está asociada con una manifestación."@es,
        "Personne, famille ou collectivité, autre qu’un producteur, un éditeur, un diffuseur ou distributeur ou bien un fabricant, associée à une manifestation."@fr ;
    rdakit:toolkitLabel "other agent associated with manifestation"@en,
        "otra persona, familia o entidad corporativa asociada con una manifestación"@es,
        "autre personne, famille ou collectivité associée à une manifestation"@fr,
        "övrig person, familj/släkt eller institution knuten till en manifestation"@sv ;
    reg:hasSubproperty <http://rdaregistry.info/Elements/m/object/P30079> ;
    reg:hasUnconstrained <http://rdaregistry.info/Elements/u/P60374> ;
    reg:lexicalAlias <http://rdaregistry.info/Elements/m/otherAgentManifestation.en> ;
    reg:name "otherAgentManifestation"@en ;
    reg:status <http://metadataregistry.org/uri/RegStatus/1001> ;
    rdfs:domain <http://rdaregistry.info/Elements/c/C10007> ;
    rdfs:isDefinedBy <http://rdaregistry.info/Elements/m/> ;
    rdfs:subPropertyOf <http://rdaregistry.info/Elements/m/P30267> ;
    skos:definition "Relates a manifestation to an agent other than a producer, publisher, distributor, or manufacturer associated with a manifestation."@en,
        "Met une manifestation en relation avec une personne, famille ou collectivité, autre qu’un producteur, un éditeur, un diffuseur ou distributeur ou bien un fabricant, associée à une manifestation."@fr ;
    skos:scopeNote "Book designers, platemakers, etc., are included."@en,
        "Comprend les graphistes, les graveurs de planches, etc."@fr .

<http://rdaregistry.info/Elements/m/P30081> a rdf:Property ;
    rdfs:label "has producer of unpublished manifestation"@en,
        "a pour producteur d’une ressource non publiée"@fr,
        "har producent av opublicerad resurs"@sv ;
    rdakit:instructionNumber "21.2" ;
    rdakit:toolkitDefinition "An agent responsible for inscribing, fabricating, constructing, etc., a manifestation in an unpublished form."@en,
        "Una persona, familia o entidad corporativa responsable de que se inscriba, fabrique o construya, etc., un recurso inédito."@es,
        "Personne, famille ou collectivité responsable de la scription, de la fabrication, de la construction, etc. d’une ressource sous une forme non publiée."@fr ;
    rdakit:toolkitLabel "producer of unpublished manifestation"@en,
        "productor de un recurso inédito"@es,
        "producteur d’une ressource non publiée"@fr,
        "producent av opublicerad resurs"@sv ;
    reg:hasSubproperty <http://rdaregistry.info/Elements/m/object/P30081> ;
    reg:hasUnconstrained <http://rdaregistry.info/Elements/u/P60440> ;
    reg:lexicalAlias <http://rdaregistry.info/Elements/m/producerOfUnpublishedManifestation.en> ;
    reg:name "producerOfUnpublishedManifestation"@en ;
    reg:status <http://metadataregistry.org/uri/RegStatus/1001> ;
    rdfs:domain <http://rdaregistry.info/Elements/c/C10007> ;
    rdfs:isDefinedBy <http://rdaregistry.info/Elements/m/> ;
    rdfs:subPropertyOf <http://rdaregistry.info/Elements/m/P30267> ;
    skos:definition "Relates a manifestation to an agent responsible for inscribing, fabricating, constructing, etc., a manifestation in an unpublished form."@en,
        "Met une manifestation en relation avec une personne, famille ou collectivité responsable de la scription, de la fabrication, de la construction, etc. d’une ressource sous une forme non publiée."@fr .

<http://rdaregistry.info/Elements/m/P30085> a rdf:Property ;
    rdfs:label "has place of distribution"@en,
        "a pour lieu de diffusion ou de distribution"@fr,
        "har distributionsort"@sv ;
    rdakit:instructionNumber "2.9.2" ;
    rdakit:toolkitDefinition "A place associated with the distribution of a manifestation in a published form."@en,
        "Un lugar asociado con la distribución de un recurso publicado."@es,
        "Lieu associé à la diffusion ou à la distribution d’une ressource sous une forme publiée."@fr ;
    rdakit:toolkitLabel "place of distribution"@en,
        "lugar de distribución"@es,
        "lieu de diffusion ou de distribution"@fr,
        "distributionsort"@sv ;
    reg:hasUnconstrained <http://rdaregistry.info/Elements/u/P60160> ;
    reg:lexicalAlias <http://rdaregistry.info/Elements/m/placeOfDistribution.en> ;
    reg:name "placeOfDistribution"@en ;
    reg:status <http://metadataregistry.org/uri/RegStatus/1001> ;
    rdfs:domain <http://rdaregistry.info/Elements/c/C10007> ;
    rdfs:isDefinedBy <http://rdaregistry.info/Elements/m/> ;
    skos:definition "Relates a manifestation to a place associated with the distribution of a manifestation in a published form."@en,
        "Met une manifestation en relation avec un lieu associé à la diffusion ou à la distribution d’une ressource sous une forme publiée."@fr .

<http://rdaregistry.info/Elements/m/P30086> a rdf:Property ;
    rdfs:label "has place of production"@en,
        "a pour lieu de production"@fr,
        "har produktionsort"@sv ;
    rdakit:instructionNumber "2.7.2" ;
    rdakit:toolkitDefinition "A place associated with the inscription, fabrication, construction, etc., of a manifestation in an unpublished form."@en,
        "Un lugar asociado con la inscripción, fabricación, construcción, etc., de un recurso en formato inédito."@es,
        "Lieu associé à la scription, la fabrication, la construction, etc. d’une ressource sous une forme non publiée."@fr ;
    rdakit:toolkitLabel "place of production"@en,
        "lugar de producción"@es,
        "lieu de production"@fr,
        "produktionsort"@sv ;
    reg:hasUnconstrained <http://rdaregistry.info/Elements/u/P60161> ;
    reg:lexicalAlias <http://rdaregistry.info/Elements/m/placeOfProduction.en> ;
    reg:name "placeOfProduction"@en ;
    reg:status <http://metadataregistry.org/uri/RegStatus/1001> ;
    rdfs:domain <http://rdaregistry.info/Elements/c/C10007> ;
    rdfs:isDefinedBy <http://rdaregistry.info/Elements/m/> ;
    skos:definition "Relates a manifestation to a place associated with the inscription, fabrication, construction, etc., of a manifestation in an unpublished form."@en,
        "Met une manifestation en relation avec un lieu associé à la scription, la fabrication, la construction, etc. d’une ressource sous une forme non publiée."@fr .

<http://rdaregistry.info/Elements/m/P30087> a rdf:Property ;
    rdfs:label "has place of manufacture"@en,
        "a pour lieu de fabrication"@fr,
        "har tillverkningsort"@sv ;
    rdakit:instructionNumber "2.10.2" ;
    rdakit:toolkitDefinition "A place associated with the printing, duplicating, casting, etc., of a manifestation in a published form."@en,
        "Un lugar asociado con la impresión, duplicación, producción, etc., de un recurso publicado."@es,
        "Lieu associé à l’impression, à la reproduction, au moulage, etc. d’une ressource sous une forme publiée."@fr ;
    rdakit:toolkitLabel "place of manufacture"@en,
        "lugar de fabricación"@es,
        "lieu de fabrication"@fr,
        "tillverkningsort"@sv ;
    reg:hasUnconstrained <http://rdaregistry.info/Elements/u/P60162> ;
    reg:lexicalAlias <http://rdaregistry.info/Elements/m/placeOfManufacture.en> ;
    reg:name "placeOfManufacture"@en ;
    reg:status <http://metadataregistry.org/uri/RegStatus/1001> ;
    rdfs:domain <http://rdaregistry.info/Elements/c/C10007> ;
    rdfs:isDefinedBy <http://rdaregistry.info/Elements/m/> ;
    skos:definition "Relates a manifestation to a place associated with the printing, duplicating, casting, etc., of a manifestation in a published form."@en,
        "Met une manifestation en relation avec un lieu associé à l’impression, à la reproduction, au moulage, etc. d’une ressource sous une forme publiée."@fr .

<http://rdaregistry.info/Elements/m/P30088> a rdf:Property ;
    rdfs:label "has place of publication"@en,
        "a pour lieu de publication"@fr,
        "har utgivningsort"@sv ;
    rdakit:instructionNumber "2.8.2" ;
    rdakit:toolkitDefinition "A place associated with the publication, release, or issuing of a manifestation."@en,
        "Un lugar asociado con la publicación, lanzamiento o edición de un recurso."@es,
        "Lieu associé à la publication, la mise à disposition ou l’édition d’une ressource."@fr ;
    rdakit:toolkitLabel "place of publication"@en,
        "lugar de publicación"@es,
        "lieu de publication"@fr,
        "utgivningsort"@sv ;
    reg:hasUnconstrained <http://rdaregistry.info/Elements/u/P60163> ;
    reg:lexicalAlias <http://rdaregistry.info/Elements/m/placeOfPublication.en> ;
    reg:name "placeOfPublication"@en ;
    reg:status <http://metadataregistry.org/uri/RegStatus/1001> ;
    rdfs:domain <http://rdaregistry.info/Elements/c/C10007> ;
    rdfs:isDefinedBy <http://rdaregistry.info/Elements/m/> ;
    skos:definition "Relates a manifestation to a place associated with the publication, release, or issuing of a manifestation."@en,
        "Met une manifestation en relation avec un lieu associé à la publication, la mise à disposition ou l’édition d’une ressource."@fr .

<http://rdaregistry.info/Elements/m/P30089> a rdf:Property ;
    rdfs:label "has parallel place of distribution"@en,
        "a pour forme parallèle du lieu de diffusion ou de distribution"@fr,
        "har parallell distributionsort"@sv ;
    rdakit:instructionNumber "2.9.3" ;
    rdakit:toolkitDefinition "A place of distribution in a language or script that differs from that recorded in a place of distribution element."@en,
        "Un lugar de distribución en una lengua y/o escritura que difiere de la registrada en el elemento lugar de distribución."@es,
        "Lieu de diffusion ou de distribution dans une langue et/ou une écriture différentes de celles enregistrées dans l’élément Lieu de diffusion ou de distribution."@fr ;
    rdakit:toolkitLabel "parallel place of distribution"@en,
        "lugar paralelo de distribución"@es,
        "forme parallèle du lieu de diffusion ou de distribution"@fr,
        "parallell distributionsort"@sv ;
    reg:hasUnconstrained <http://rdaregistry.info/Elements/u/P60164> ;
    reg:lexicalAlias <http://rdaregistry.info/Elements/m/parallelPlaceOfDistribution.en> ;
    reg:name "parallelPlaceOfDistribution"@en ;
    reg:status <http://metadataregistry.org/uri/RegStatus/1001> ;
    rdfs:domain <http://rdaregistry.info/Elements/c/C10007> ;
    rdfs:isDefinedBy <http://rdaregistry.info/Elements/m/> ;
    skos:definition "Relates a manifestation to a place of distribution in a language or script that differs from that recorded in a place of distribution element."@en,
        "Met une manifestation en relation avec un lieu de diffusion ou de distribution dans une langue et/ou une écriture différentes de celles enregistrées dans l’élément Lieu de diffusion ou de distribution."@fr .

<http://rdaregistry.info/Elements/m/P30090> a rdf:Property ;
    rdfs:label "has parallel place of manufacture"@en,
        "a pour forme parallèle du lieu de fabrication"@fr,
        "har parallell tillverkningsort"@sv ;
    rdakit:instructionNumber "2.10.3" ;
    rdakit:toolkitDefinition "A place of manufacture in a language or script that differs from that recorded in a place of manufacture element."@en,
        "Un lugar de fabricación en una lengua y/o escritura que difiere de la registrada en el elemento lugar de fabricación"@es,
        "Lieu de fabrication dans une langue et/ou une écriture différentes de celles enregistrées dans l’élément Lieu de fabrication."@fr ;
    rdakit:toolkitLabel "parallel place of manufacture"@en,
        "lugar paralelo de fabricación"@es,
        "forme parallèle du lieu de fabrication"@fr,
        "parallell tillverkningsort"@sv ;
    reg:hasUnconstrained <http://rdaregistry.info/Elements/u/P60165> ;
    reg:lexicalAlias <http://rdaregistry.info/Elements/m/parallelPlaceOfManufacture.en> ;
    reg:name "parallelPlaceOfManufacture"@en ;
    reg:status <http://metadataregistry.org/uri/RegStatus/1001> ;
    rdfs:domain <http://rdaregistry.info/Elements/c/C10007> ;
    rdfs:isDefinedBy <http://rdaregistry.info/Elements/m/> ;
    skos:definition "Relates a manifestation to a place of manufacture in a language or script that differs from that recorded in a place of manufacture element."@en,
        "Met une manifestation en relation avec un lieu de fabrication dans une langue et/ou une écriture différentes de celles enregistrées dans l’élément Lieu de fabrication."@fr .

<http://rdaregistry.info/Elements/m/P30091> a rdf:Property ;
    rdfs:label "has parallel place of production"@en,
        "a pour forme parallèle du lieu de production"@fr,
        "har parallell produktionsort"@sv ;
    rdakit:instructionNumber "2.7.3" ;
    rdakit:toolkitDefinition "A place of production in a language or script that differs from that recorded in a place of production element."@en,
        "Un lugar de producción en una lengua y/o escritura que difiere de la registrada en el elemento lugar de producción."@es,
        "Lieu de production dans une langue et/ou une écriture différentes de celles enregistrées dans l’élément Lieu de production."@fr ;
    rdakit:toolkitLabel "parallel place of production"@en,
        "lugar paralelo de producción"@es,
        "forme parallèle du lieu de production"@fr,
        "parallell produktionsort"@sv ;
    reg:hasUnconstrained <http://rdaregistry.info/Elements/u/P60166> ;
    reg:lexicalAlias <http://rdaregistry.info/Elements/m/parallelPlaceOfProduction.en> ;
    reg:name "parallelPlaceOfProduction"@en ;
    reg:status <http://metadataregistry.org/uri/RegStatus/1001> ;
    rdfs:domain <http://rdaregistry.info/Elements/c/C10007> ;
    rdfs:isDefinedBy <http://rdaregistry.info/Elements/m/> ;
    skos:definition "Relates a manifestation to a place of production in a language or script that differs from that recorded in a place of production element."@en,
        "Met une manifestation en relation avec un lieu de production dans une langue et/ou une écriture différentes de celles enregistrées dans l’élément Lieu de production."@fr .

<http://rdaregistry.info/Elements/m/P30092> a rdf:Property ;
    rdfs:label "has parallel place of publication"@en,
        "a pour forme parallèle du lieu de publication"@fr,
        "har parallell utgivningsort"@sv ;
    rdakit:instructionNumber "2.8.3" ;
    rdakit:toolkitDefinition "A place of publication in a language or script that differs from that recorded in a place of publication element."@en,
        "Un lugar de publicación en una lengua y/o escritura que difiere de la registrada en el elemento lugar de publicación"@es,
        "Lieu de publication dans une langue et/ou une écriture différentes de celles enregistrées dans l’élément Lieu de publication."@fr ;
    rdakit:toolkitLabel "parallel place of publication"@en,
        "lugar paralelo de publicación"@es,
        "forme parallèle du lieu de publication"@fr,
        "parallell utgivningsort"@sv ;
    reg:hasUnconstrained <http://rdaregistry.info/Elements/u/P60167> ;
    reg:lexicalAlias <http://rdaregistry.info/Elements/m/parallelPlaceOfPublication.en> ;
    reg:name "parallelPlaceOfPublication"@en ;
    reg:status <http://metadataregistry.org/uri/RegStatus/1001> ;
    rdfs:domain <http://rdaregistry.info/Elements/c/C10007> ;
    rdfs:isDefinedBy <http://rdaregistry.info/Elements/m/> ;
    skos:definition "Relates a manifestation to a place of publication in a language or script that differs from that recorded in a place of publication element."@en,
        "Met une manifestation en relation avec un lieu de publication dans une langue et/ou une écriture différentes de celles enregistrées dans l’élément Lieu de publication."@fr .

<http://rdaregistry.info/Elements/m/P30094> a rdf:Property ;
    rdfs:label "has parallel producer’s name"@en,
        "a pour forme parallèle du nom du producteur"@fr,
        "har parallellt producentnamn"@sv ;
    rdakit:instructionNumber "2.7.5" ;
    rdakit:toolkitDefinition "A producer's name in a language or script that differs from that recorded in a producer's name element."@en,
        "Un nombre de productor en una lengua y/o escritura que difiere de la registrada en el elemento nombre del productor."@es,
        "Nom du producteur dans une langue et/ou une écriture différentes de celles enregistrées dans l’élément Nom du producteur."@fr ;
    rdakit:toolkitLabel "parallel producer's name"@en,
        "nombre paralelo del productor"@es,
        "forme parallèle du nom du producteur"@fr,
        "parallellt producentnamn"@sv ;
    reg:hasUnconstrained <http://rdaregistry.info/Elements/u/P60172> ;
    reg:lexicalAlias <http://rdaregistry.info/Elements/m/parallelProducersName.en> ;
    reg:name "parallelProducersName"@en ;
    reg:status <http://metadataregistry.org/uri/RegStatus/1001> ;
    rdfs:domain <http://rdaregistry.info/Elements/c/C10007> ;
    rdfs:isDefinedBy <http://rdaregistry.info/Elements/m/> ;
    skos:definition "Relates a manifestation to a producer's name in a language or script that differs from that recorded in a producer's name element."@en,
        "Met une manifestation en relation avec un nom du producteur dans une langue et/ou une écriture différentes de celles enregistrées dans l’élément Nom du producteur."@fr .

<http://rdaregistry.info/Elements/m/P30095> a rdf:Property ;
    rdfs:label "has parallel publisher’s name"@en,
        "a pour forme parallèle du nom de l’éditeur"@fr,
        "har parallellt utgivarnamn"@sv ;
    rdakit:instructionNumber "2.8.5" ;
    rdakit:toolkitDefinition "A publisher's name in a language or script that differs from that recorded in a publisher's name element."@en,
        "Un nombre del editor en una lengua y/o escritura que difiere de la registrada en el elemento nombre del editor."@es,
        "Nom d’éditeur dans une langue et/ou une écriture différentes de celles enregistrées dans l’élément Nom d’éditeur."@fr ;
    rdakit:toolkitLabel "parallel publisher's name"@en,
        "nombre paralelo del editor"@es,
        "forme parallèle du nom de l’éditeur"@fr,
        "parallellt utgivarnamn"@sv ;
    reg:hasUnconstrained <http://rdaregistry.info/Elements/u/P60173> ;
    reg:lexicalAlias <http://rdaregistry.info/Elements/m/parallelPublishersName.en> ;
    reg:name "parallelPublishersName"@en ;
    reg:status <http://metadataregistry.org/uri/RegStatus/1001> ;
    rdfs:domain <http://rdaregistry.info/Elements/c/C10007> ;
    rdfs:isDefinedBy <http://rdaregistry.info/Elements/m/> ;
    skos:definition "Relates a manifestation to a publisher's name in a language or script that differs from that recorded in a publisher's name element."@en,
        "Met une manifestation en relation avec un nom d’éditeur dans une langue et/ou une écriture différentes de celles enregistrées dans l’élément Nom d’éditeur."@fr .

<http://rdaregistry.info/Elements/m/P30103> a rdf:Property ;
    rdfs:label "has exemplar of manifestation"@en,
        "a pour exemplaire d’une manifestation"@fr,
        "har exemplar av manifestation"@sv ;
    rdakit:instructionNumber "17.11" ;
    rdakit:toolkitDefinition "A single exemplar or instance of a manifestation."@en,
        "Un ejemplar individual o una instancia de una manifestación."@es,
        "Exemplaire isolé ou instance d’une manifestation."@fr ;
    rdakit:toolkitLabel "exemplar of manifestation"@en,
        "ejemplar de una manifestación"@es,
        "exemplaire d’une manifestation"@fr,
        "exemplar av manifestation"@sv ;
    reg:hasSubproperty <http://rdaregistry.info/Elements/m/object/P30103> ;
    reg:lexicalAlias <http://rdaregistry.info/Elements/m/exemplarOfManifestation.en> ;
    reg:name "exemplarOfManifestation"@en ;
    reg:status <http://metadataregistry.org/uri/RegStatus/1001> ;
    rdfs:domain <http://rdaregistry.info/Elements/c/C10007> ;
    rdfs:isDefinedBy <http://rdaregistry.info/Elements/m/> ;
    skos:definition "Relates a manifestation to a single exemplar or instance of a manifestation."@en,
        "Met une manifestation en relation avec un exemplaire isolé ou une instance d’une manifestation."@fr .

<http://rdaregistry.info/Elements/m/P30106> a rdf:Property ;
    rdfs:label "has series statement"@en,
        "a pour mention de collection"@fr,
        "har serieuppgift"@sv ;
    rdakit:instructionNumber "2.12" ;
    rdakit:toolkitDefinition "A statement identifying a series to which a manifestation belongs and a numbering of a manifestation within the series."@en,
        "Una mención que identifica una serie a la que pertenece un recurso y la numeración del recurso dentro de la serie."@es,
        "Mention identifiant une collection à laquelle une ressource appartient et la numérotation de la ressource à l’intérieur de la collection."@fr ;
    rdakit:toolkitLabel "series statement"@en,
        "mención de serie"@es,
        "mention de collection"@fr,
        "serieuppgift"@sv ;
    reg:hasUnconstrained <http://rdaregistry.info/Elements/u/P60328> ;
    reg:lexicalAlias <http://rdaregistry.info/Elements/m/seriesStatement.en> ;
    reg:name "seriesStatement"@en ;
    reg:status <http://metadataregistry.org/uri/RegStatus/1001> ;
    rdfs:domain <http://rdaregistry.info/Elements/c/C10007> ;
    rdfs:isDefinedBy <http://rdaregistry.info/Elements/m/> ;
    skos:definition "Relates a manifestation to a statement identifying a series to which a manifestation belongs and a numbering of a manifestation within the series."@en,
        "Met une manifestation en relation avec une mention identifiant une collection à laquelle une ressource appartient et la numérotation de la ressource à l’intérieur de la collection."@fr ;
    skos:scopeNote "A series statement may also include information identifying one or more subseries to which the resource being described belongs. A series statement sometimes includes statements of responsibility relating to a series or subseries."@en,
        "Une mention de collection peut aussi comprendre l’information identifiant une ou plusieurs sous-collections auxquelles la ressource décrite appartient. Les mentions de collection comprennent parfois des mentions de responsabilité relatives à une collection ou une sous-collection."@fr .

<http://rdaregistry.info/Elements/m/P30107> a rdf:Property ;
    rdfs:label "has edition statement"@en,
        "a pour mention d’édition"@fr,
        "har upplageuppgift"@sv ;
    rdakit:instructionNumber "2.5" ;
    rdakit:toolkitDefinition "A statement identifying an edition to which a manifestation belongs."@en,
        "Una mención que identifica la edición a la que pertenece un recurso."@es,
        "Mention identifiant l’édition à laquelle appartient la ressource."@fr ;
    rdakit:toolkitLabel "edition statement"@en,
        "mención de edición"@es,
        "mention d’édition"@fr,
        "upplageuppgift"@sv ;
    reg:hasUnconstrained <http://rdaregistry.info/Elements/u/P60329> ;
    reg:lexicalAlias <http://rdaregistry.info/Elements/m/editionStatement.en> ;
    reg:name "editionStatement"@en ;
    reg:status <http://metadataregistry.org/uri/RegStatus/1001> ;
    rdfs:domain <http://rdaregistry.info/Elements/c/C10007> ;
    rdfs:isDefinedBy <http://rdaregistry.info/Elements/m/> ;
    skos:definition "Relates a manifestation to a statement identifying an edition to which a manifestation belongs."@en,
        "Met une manifestation en relation avec une mention identifiant l’édition à laquelle appartient la ressource."@fr ;
    skos:scopeNote "An edition statement sometimes includes a designation of a named revision of an edition. An edition statement sometimes includes a statement of responsibility relating to the edition or to a named revision of an edition."@en,
        "Une mention d’édition comprend parfois une indication d’une révision nommée d’une édition. Une mention d’édition comprend parfois une ou plusieurs mentions de responsabilité relatives à l’édition et/ou à une révision nommée d’une édition."@fr .

<http://rdaregistry.info/Elements/m/P30108> a rdf:Property ;
    rdfs:label "has distribution statement"@en,
        "a pour mention de diffusion ou de distribution"@fr,
        "har distributionsuppgift"@sv ;
    rdakit:instructionNumber "2.9" ;
    rdakit:toolkitDefinition "A statement identifying a place or places of distribution, distributor or distributors, and date or dates of distribution of a manifestation in a published form."@en,
        "Una mención que identifica el lugar o lugares de distribución, el distribuidor o distribuidores, y la fecha o fechas de publicación de un recurso en forma publicada."@es,
        "Mention identifiant le ou les lieux de diffusion ou de distribution, le ou les diffuseurs ou distributeurs et la ou les dates de diffusion ou de distribution d’une ressource sous une forme publiée."@fr ;
    rdakit:toolkitLabel "distribution statement"@en,
        "mención de distribución"@es,
        "mention de diffusion ou de distribution"@fr,
        "distributionsuppgift"@sv ;
    reg:hasUnconstrained <http://rdaregistry.info/Elements/u/P60330> ;
    reg:lexicalAlias <http://rdaregistry.info/Elements/m/distributionStatement.en> ;
    reg:name "distributionStatement"@en ;
    reg:status <http://metadataregistry.org/uri/RegStatus/1001> ;
    rdfs:domain <http://rdaregistry.info/Elements/c/C10007> ;
    rdfs:isDefinedBy <http://rdaregistry.info/Elements/m/> ;
    skos:definition "Relates a manifestation to a statement identifying a place or places of distribution, distributor or distributors, and date or dates of distribution of a manifestation in a published form."@en,
        "Met une manifestation en relation avec une mention identifiant le ou les lieux de diffusion ou de distribution, le ou les diffuseurs ou distributeurs et la ou les dates de diffusion ou de distribution d’une ressource sous une forme publiée."@fr .

<http://rdaregistry.info/Elements/m/P30109> a rdf:Property ;
    rdfs:label "has manufacture statement"@en,
        "a pour mention de fabrication"@fr,
        "har tillverkningsuppgift"@sv ;
    rdakit:instructionNumber "2.10" ;
    rdakit:toolkitDefinition "A statement identifying a place or places of manufacture, manufacturer or manufacturers, and date or dates of manufacture of a manifestation in a published form."@en,
        "Una mención que identifica el lugar o lugares de fabricación, el fabricante o fabricantes, y la fecha o fechas de fabricación de un recurso impreso."@es,
        "Mention identifiant le ou les lieux de fabrication, le ou les fabricants et la ou les dates de fabrication d’une ressource sous une forme publiée."@fr ;
    rdakit:toolkitLabel "manufacture statement"@en,
        "mención de fabricación"@es,
        "mention de fabrication"@fr,
        "tillverkningsuppgift"@sv ;
    reg:hasUnconstrained <http://rdaregistry.info/Elements/u/P60331> ;
    reg:lexicalAlias <http://rdaregistry.info/Elements/m/manufactureStatement.en> ;
    reg:name "manufactureStatement"@en ;
    reg:status <http://metadataregistry.org/uri/RegStatus/1001> ;
    rdfs:domain <http://rdaregistry.info/Elements/c/C10007> ;
    rdfs:isDefinedBy <http://rdaregistry.info/Elements/m/> ;
    skos:definition "Relates a manifestation to a statement identifying a place or places of manufacture, manufacturer or manufacturers, and date or dates of manufacture of a manifestation in a published form."@en,
        "Met une manifestation en relation avec une mention identifiant le ou les lieux de fabrication, le ou les fabricants et la ou les dates de fabrication d’une ressource sous une forme publiée."@fr ;
    skos:scopeNote "Manufacture statements include statements relating to the printing, duplicating, casting, etc., of a manifestation in a published form."@en,
        "Les mentions de fabrication comprennent les mentions relatives à l’impression, à la reproduction, au moulage, etc. d’une ressource sous une forme publiée."@fr .

<http://rdaregistry.info/Elements/m/P30110> a rdf:Property ;
    rdfs:label "has production statement"@en,
        "a pour mention de production"@fr,
        "har produktionsuppgift"@sv ;
    rdakit:instructionNumber "2.7" ;
    rdakit:toolkitDefinition "A statement identifying a place or places of production, producer or producers, and date or dates of production of a manifestation in an unpublished form."@en,
        "Una mención que identifica el lugar o lugares de producción, el productor o productores, y la fecha o fechas de producción de un recurso en un formato inédito."@es,
        "Mention identifiant le ou les lieux de production, le ou les producteurs et la ou les dates de production d’une ressource sous une forme non publiée."@fr ;
    rdakit:toolkitLabel "production statement"@en,
        "mención de producción"@es,
        "mention de production"@fr,
        "produktionsuppgift"@sv ;
    reg:hasUnconstrained <http://rdaregistry.info/Elements/u/P60332> ;
    reg:lexicalAlias <http://rdaregistry.info/Elements/m/productionStatement.en> ;
    reg:name "productionStatement"@en ;
    reg:status <http://metadataregistry.org/uri/RegStatus/1001> ;
    rdfs:domain <http://rdaregistry.info/Elements/c/C10007> ;
    rdfs:isDefinedBy <http://rdaregistry.info/Elements/m/> ;
    skos:definition "Relates a manifestation to a statement identifying a place or places of production, producer or producers, and date or dates of production of a manifestation in an unpublished form."@en,
        "Met une manifestation en relation avec une mention identifiant le ou les lieux de production, le ou les producteurs et la ou les dates de production d’une ressource sous une forme non publiée."@fr ;
    skos:scopeNote "Production statements include statements relating to the inscription, fabrication, construction, etc., of a manifestation in an unpublished form."@en,
        "Les mentions de production comprennent les mentions relatives à la scription, à la fabrication, à la construction, etc. d’une ressource sous une forme non publiée."@fr .

<http://rdaregistry.info/Elements/m/P30111> a rdf:Property ;
    rdfs:label "has publication statement"@en,
        "a pour mention de publication"@fr,
        "har utgivningsuppgift"@sv ;
    rdakit:instructionNumber "2.8" ;
    rdakit:toolkitDefinition "A statement identifying a place or places of publication, publisher or publishers, and date or dates of publication of a manifestation."@en,
        "Una mención que identifica el lugar o lugares de publicación, el editor o los editores, y la fecha o fechas de publicación de un recurso."@es,
        "Mention identifiant le ou les lieux de publication, le ou les éditeurs et la ou les dates de publication d’une ressource."@fr ;
    rdakit:toolkitLabel "publication statement"@en,
        "mención de publicación"@es,
        "mention de publication"@fr,
        "utgivningsuppgift"@sv ;
    reg:hasUnconstrained <http://rdaregistry.info/Elements/u/P60333> ;
    reg:lexicalAlias <http://rdaregistry.info/Elements/m/publicationStatement.en> ;
    reg:name "publicationStatement"@en ;
    reg:status <http://metadataregistry.org/uri/RegStatus/1001> ;
    rdfs:domain <http://rdaregistry.info/Elements/c/C10007> ;
    rdfs:isDefinedBy <http://rdaregistry.info/Elements/m/> ;
    skos:definition "Relates a manifestation to a statement identifying a place or places of publication, publisher or publishers, and date or dates of publication of a manifestation."@en,
        "Met une manifestation en relation avec une mention identifiant le ou les lieux de publication, le ou les éditeurs et la ou les dates de publication d’une ressource."@fr ;
    skos:scopeNote "Publication statements include statements relating to the publication, release, or issuing of a manifestation."@en,
        "Les mentions de publication comprennent les mentions relatives à la publication, à la mise à disposition ou à l’émission d’une ressource."@fr .

<http://rdaregistry.info/Elements/m/P30112> a rdf:Property ;
    rdfs:label "has parallel statement of responsibility relating to named revision of edition"@en,
        "a pour mention de responsabilité parallèle relative à une révision nommée d’une édition"@fr,
        "har parallell upphovsuppgift som hänför sig till påföljande upplagebeteckning"@sv ;
    rdakit:instructionNumber "2.5.9" ;
    rdakit:toolkitDefinition "A statement of responsibility relating to a named revision of an edition in a language or script that differs from that recorded in a statement of responsibility relating to a named revision of an edition element."@en,
        "Una mención de responsabilidad relacionada con una revisión mencionada de una edición en una lengua y/o escritura que difiere de la registrada en la mención de responsabilidad relacionada con el elemento revisión mencionada de una edición."@es,
        "Mention de responsabilité relative à une révision nommée d’une édition dans une langue et/ou une écriture différentes de celles enregistrées dans l’élément Mention de responsabilité relative à une révision nommée d’une édition."@fr ;
    rdakit:toolkitLabel "parallel statement of responsibility relating to named revision of edition"@en,
        "mención paralela de responsabilidad relacionada con una revisión mencionada de una edición"@es,
        "mention de responsabilité parallèle relative à une révision nommée d’une édition"@fr,
        "parallell upphovsuppgift som hänför sig till påföljande upplagebeteckning"@sv ;
    reg:hasUnconstrained <http://rdaregistry.info/Elements/u/P60334> ;
    reg:lexicalAlias <http://rdaregistry.info/Elements/m/parallelStatementOfResponsibilityRelatingToNamedRevisionOfEdition.en> ;
    reg:name "parallelStatementOfResponsibilityRelatingToNamedRevisionOfEdition"@en ;
    reg:status <http://metadataregistry.org/uri/RegStatus/1001> ;
    rdfs:domain <http://rdaregistry.info/Elements/c/C10007> ;
    rdfs:isDefinedBy <http://rdaregistry.info/Elements/m/> ;
    skos:definition "Relates a manifestation to a statement of responsibility relating to a named revision of an edition in a language or script that differs from that recorded in a statement of responsibility relating to a named revision of an edition element."@en,
        "Met une manifestation en relation avec une mention de responsabilité relative à une révision nommée d’une édition dans une langue et/ou une écriture différentes de celles enregistrées dans l’élément Mention de responsabilité relative à une révision nommée d’une édition."@fr .

<http://rdaregistry.info/Elements/m/P30113> a rdf:Property ;
    rdfs:label "has parallel statement of responsibility relating to series"@en,
        "a pour mention de responsabilité parallèle relative à la collection"@fr,
        "har parallell upphovsuppgift till serie"@sv ;
    rdakit:instructionNumber "2.12.7" ;
    rdakit:toolkitDefinition "A statement of responsibility relating to series in a language or script that differs from that recorded in a statement of responsibility relating to series element."@en,
        "Una mención de responsabilidad relacionada con la serie en una lengua y/o escritura que difiere de la registrada en el elemento mención de responsabilidad relacionada con la serie."@es,
        "Mention de responsabilité relative à la collection dans une langue et/ou une écriture différentes de celles enregistrées dans l’élément Mention de responsabilité relative à la collection."@fr ;
    rdakit:toolkitLabel "parallel statement of responsibility relating to series"@en,
        "mención paralela de responsabilidad relacionada con la serie"@es,
        "mention de responsabilité parallèle relative à la collection"@fr,
        "parallell upphovsuppgift till serie"@sv ;
    reg:hasUnconstrained <http://rdaregistry.info/Elements/u/P60335> ;
    reg:lexicalAlias <http://rdaregistry.info/Elements/m/parallelStatementOfResponsibilityRelatingToSeries.en> ;
    reg:name "parallelStatementOfResponsibilityRelatingToSeries"@en ;
    reg:status <http://metadataregistry.org/uri/RegStatus/1001> ;
    rdfs:domain <http://rdaregistry.info/Elements/c/C10007> ;
    rdfs:isDefinedBy <http://rdaregistry.info/Elements/m/> ;
    skos:definition "Relates a manifestation to a statement of responsibility relating to series in a language or script that differs from that recorded in a statement of responsibility relating to series element."@en,
        "Met une manifestation en relation avec une mention de responsabilité relative à la collection dans une langue et/ou une écriture différentes de celles enregistrées dans l’élément Mention de responsabilité relative à la collection."@fr .

<http://rdaregistry.info/Elements/m/P30114> a rdf:Property ;
    rdfs:label "has parallel statement of responsibility relating to subseries"@en,
        "a pour mention de responsabilité parallèle relative à la sous-collection"@fr,
        "har parallell upphovsuppgift till underserie"@sv ;
    rdakit:instructionNumber "2.12.15" ;
    rdakit:toolkitDefinition "A statement of responsibility relating to subseries in a language or script that differs from that recorded in a statement of responsibility relating to subseries element."@en,
        "Una mención de responsabilidad relacionada con una subserie en una lengua y/o escritura que difiere de la registrada en el elemento mención de responsabilidad relacionada con la subserie."@es,
        "Mention de responsabilité relative à la sous-collection dans une langue et/ou une écriture différentes de celles enregistrées dans l’élément Mention de responsabilité relative à la sous-collection."@fr ;
    rdakit:toolkitLabel "parallel statement of responsibility relating to subseries"@en,
        "mención paralela de responsabilidad relacionada con la subserie"@es,
        "mention de responsabilité parallèle relative à la sous-collection"@fr,
        "parallell upphovsuppgift till underserie"@sv ;
    reg:hasUnconstrained <http://rdaregistry.info/Elements/u/P60336> ;
    reg:lexicalAlias <http://rdaregistry.info/Elements/m/parallelStatementOfResponsibilityRelatingToSubseries.en> ;
    reg:name "parallelStatementOfResponsibilityRelatingToSubseries"@en ;
    reg:status <http://metadataregistry.org/uri/RegStatus/1001> ;
    rdfs:domain <http://rdaregistry.info/Elements/c/C10007> ;
    rdfs:isDefinedBy <http://rdaregistry.info/Elements/m/> ;
    skos:definition "Relates a manifestation to a statement of responsibility relating to subseries in a language or script that differs from that recorded in a statement of responsibility relating to subseries element."@en,
        "Met une manifestation en relation avec une mention de responsabilité relative à la sous-collection dans une langue et/ou une écriture différentes de celles enregistrées dans l’élément Mention de responsabilité relative à la sous-collection."@fr .

<http://rdaregistry.info/Elements/m/P30115> a rdf:Property ;
    rdfs:label "has parallel statement of responsibility relating to edition"@en,
        "a pour mention de responsabilité parallèle relative à l’édition"@fr,
        "har parallell upphovsuppgift som hänför sig till upplagan"@sv ;
    rdakit:instructionNumber "2.5.5" ;
    rdakit:toolkitDefinition "A statement of responsibility relating to the edition in a language or script that differs from that recorded in a statement of responsibility relating to the edition element."@en,
        "Una mención de responsabilidad relacionada con la edición en una lengua y/o escritura que difiere de la registrada en la mención de responsabilidad relacionada con el elemento edición"@es,
        "Mention de responsabilité relative à l’édition dans une langue et/ou une écriture différentes de celles enregistrées dans l’élément Mention de responsabilité relative à l’édition."@fr ;
    rdakit:toolkitLabel "parallel statement of responsibility relating to edition"@en,
        "mención paralela de responsabilidad relacionada con la edición"@es,
        "mention de responsabilité parallèle relative à l’édition"@fr,
        "parallell upphovsuppgift som hänför sig till upplagan"@sv ;
    reg:hasUnconstrained <http://rdaregistry.info/Elements/u/P60337> ;
    reg:lexicalAlias <http://rdaregistry.info/Elements/m/parallelStatementOfResponsibilityRelatingToEdition.en> ;
    reg:name "parallelStatementOfResponsibilityRelatingToEdition"@en ;
    reg:status <http://metadataregistry.org/uri/RegStatus/1001> ;
    rdfs:domain <http://rdaregistry.info/Elements/c/C10007> ;
    rdfs:isDefinedBy <http://rdaregistry.info/Elements/m/> ;
    skos:definition "Relates a manifestation to a statement of responsibility relating to the edition in a language or script that differs from that recorded in a statement of responsibility relating to the edition element."@en,
        "Met une manifestation en relation avec une mention de responsabilité relative à l’édition dans une langue et/ou une écriture différentes de celles enregistrées dans l’élément Mention de responsabilité relative à l’édition."@fr .

<http://rdaregistry.info/Elements/m/P30118> a rdf:Property ;
    rdfs:label "has statement of responsibility relating to named revision of edition"@en,
        "a pour mention de responsabilité relative à une révision nommée d’une édition"@fr,
        "har upphovsuppgift som hänför sig till påföljande upplageuppgift"@sv ;
    rdakit:instructionNumber "2.5.8" ;
    rdakit:toolkitDefinition "A statement relating to the identification of agents responsible for a named revision of an edition."@en,
        "Una mención relacionada con la identificación de todas las personas, familias o entidades corporativas responsables de una revisión mencionada de una edición."@es,
        "Mention relative à l’identification de toute personne, famille ou collectivité responsable de la révision nommée d’une édition."@fr ;
    rdakit:toolkitLabel "statement of responsibility relating to named revision of edition"@en,
        "mención de responsabilidad relacionada con una revisión mencionada de una edición"@es,
        "mention de responsabilité relative à une révision nommée d’une édition"@fr,
        "upphovsuppgift som hänför sig till påföljande upplageuppgift"@sv ;
    reg:hasUnconstrained <http://rdaregistry.info/Elements/u/P60340> ;
    reg:lexicalAlias <http://rdaregistry.info/Elements/m/statementOfResponsibilityRelatingToNamedRevisionOfEdition.en> ;
    reg:name "statementOfResponsibilityRelatingToNamedRevisionOfEdition"@en ;
    reg:status <http://metadataregistry.org/uri/RegStatus/1001> ;
    rdfs:domain <http://rdaregistry.info/Elements/c/C10007> ;
    rdfs:isDefinedBy <http://rdaregistry.info/Elements/m/> ;
    skos:definition "Relates a manifestation to a statement relating to the identification of agents responsible for a named revision of an edition."@en,
        "Met une manifestation en relation avec une mention relative à l’identification de toute personne, famille ou collectivité responsable de la révision nommée d’une édition."@fr .

<http://rdaregistry.info/Elements/m/P30119> a rdf:Property ;
    rdfs:label "has statement of responsibility relating to series"@en,
        "a pour mention de responsabilité relative à la collection"@fr,
        "har upphovsuppgift till serie"@sv ;
    rdakit:instructionNumber "2.12.6" ;
    rdakit:toolkitDefinition "A statement relating to the identification of agents responsible for a series."@en,
        "Una mención relacionada con la identificación de personas, familias o entidades corporativas responsables de una serie."@es,
        "Mention relative à l’identification de toute personne, famille ou collectivité responsable d’une collection."@fr ;
    rdakit:toolkitLabel "statement of responsibility relating to series"@en,
        "mención de responsabilidad relacionada con la serie"@es,
        "mention de responsabilité relative à la collection"@fr,
        "upphovsuppgift till serie"@sv ;
    reg:hasUnconstrained <http://rdaregistry.info/Elements/u/P60341> ;
    reg:lexicalAlias <http://rdaregistry.info/Elements/m/statementOfResponsibilityRelatingToSeries.en> ;
    reg:name "statementOfResponsibilityRelatingToSeries"@en ;
    reg:status <http://metadataregistry.org/uri/RegStatus/1001> ;
    rdfs:domain <http://rdaregistry.info/Elements/c/C10007> ;
    rdfs:isDefinedBy <http://rdaregistry.info/Elements/m/> ;
    skos:definition "Relates a manifestation to a statement relating to the identification of agents responsible for a series."@en,
        "Met une manifestation en relation avec une mention relative à l’identification de toute personne, famille ou collectivité responsable d’une collection."@fr .

<http://rdaregistry.info/Elements/m/P30120> a rdf:Property ;
    rdfs:label "has statement of responsibility relating to subseries"@en,
        "a pour mention de responsabilité relative à la sous-collection"@fr,
        "har upphovsuppgift till underserie"@sv ;
    rdakit:instructionNumber "2.12.14" ;
    rdakit:toolkitDefinition "A statement relating to the identification of agents responsible for a subseries."@en,
        "Una mención relacionada con la identificación de personas, familias o entidades corporativas responsables por una subserie."@es,
        "Mention relative à l’identification de toute personne, famille ou collectivité responsable d’une sous-collection."@fr ;
    rdakit:toolkitLabel "statement of responsibility relating to subseries"@en,
        "mención de responsabilidad relacionada con la subserie"@es,
        "mention de responsabilité relative à la sous-collection"@fr,
        "upphovsuppgift till underserie"@sv ;
    reg:hasUnconstrained <http://rdaregistry.info/Elements/u/P60342> ;
    reg:lexicalAlias <http://rdaregistry.info/Elements/m/statementOfResponsibilityRelatingToSubseries.en> ;
    reg:name "statementOfResponsibilityRelatingToSubseries"@en ;
    reg:status <http://metadataregistry.org/uri/RegStatus/1001> ;
    rdfs:domain <http://rdaregistry.info/Elements/c/C10007> ;
    rdfs:isDefinedBy <http://rdaregistry.info/Elements/m/> ;
    skos:definition "Relates a manifestation to a statement relating to the identification of agents responsible for a subseries."@en,
        "Met une manifestation en relation avec une mention relative à l’identification de toute personne, famille ou collectivité responsable d’une sous-collection."@fr .

<http://rdaregistry.info/Elements/m/P30121> a rdf:Property ;
    rdfs:label "has statement of responsibility relating to edition"@en,
        "a pour mention de responsabilité relative à l’édition"@fr,
        "har upplagespecifik upphovsuppgift"@sv ;
    rdakit:instructionNumber "2.5.4" ;
    rdakit:toolkitDefinition "A statement relating to the identification of agents responsible for an edition being described but not to all editions."@en,
        "Una mención relacionada con la identificación de las personas, familias o entidades corporativas responsables de la edición descrita, pero no de todas las ediciones."@es,
        "Mention relative à l’identification de toute personne, famille ou collectivité responsable de l’édition décrite mais pas de toutes les éditions."@fr ;
    rdakit:toolkitLabel "statement of responsibility relating to edition"@en,
        "mención de responsabilidad relacionada con la edición"@es,
        "mention de responsabilité relative à l’édition"@fr,
        "upplagespecifik upphovsuppgift"@sv ;
    reg:hasUnconstrained <http://rdaregistry.info/Elements/u/P60343> ;
    reg:lexicalAlias <http://rdaregistry.info/Elements/m/statementOfResponsibilityRelatingToEdition.en> ;
    reg:name "statementOfResponsibilityRelatingToEdition"@en ;
    reg:status <http://metadataregistry.org/uri/RegStatus/1001> ;
    rdfs:domain <http://rdaregistry.info/Elements/c/C10007> ;
    rdfs:isDefinedBy <http://rdaregistry.info/Elements/m/> ;
    skos:definition "Relates a manifestation to a statement relating to the identification of agents responsible for an edition being described but not to all editions."@en,
        "Met une manifestation en relation avec une mention relative à l’identification de toute personne, famille ou collectivité responsable de l’édition décrite mais pas de toutes les éditions."@fr .

<http://rdaregistry.info/Elements/m/P30129> a rdf:Property ;
    rdfs:label "has later title proper"@en,
        "a pour titre propre ultérieur"@fr,
        "har efterföljande huvudtitel"@sv ;
    rdakit:instructionNumber "2.3.8" ;
    rdakit:toolkitDefinition "A title proper appearing on a later issue or part of a multipart monograph or serial that differs from that on the first or earliest issue or part."@en,
        "Un título propiamente dicho que aparece en una entrega o parte posterior de una monografía en varias partes o publicación seriada que difiere del de la primera o anterior entrega o parte."@es,
        "Titre propre figurant sur une livraison ou partie ultérieure d’une monographie en plusieurs parties ou d’une publication en série et qui diffère de celui figurant sur la première ou la plus ancienne livraison ou partie."@fr ;
    rdakit:toolkitLabel "later title proper"@en,
        "título propiamente dicho posterior"@es,
        "titre propre ultérieur"@fr,
        "efterföljande huvudtitel"@sv ;
    reg:hasUnconstrained <http://rdaregistry.info/Elements/u/P60357> ;
    reg:lexicalAlias <http://rdaregistry.info/Elements/m/laterTitleProper.en> ;
    reg:name "laterTitleProper"@en ;
    reg:status <http://metadataregistry.org/uri/RegStatus/1001> ;
    rdfs:domain <http://rdaregistry.info/Elements/c/C10007> ;
    rdfs:isDefinedBy <http://rdaregistry.info/Elements/m/> ;
    rdfs:subPropertyOf <http://rdaregistry.info/Elements/m/P30156> ;
    skos:definition "Relates a manifestation to a title proper appearing on a later issue or part of a multipart monograph or serial that differs from that on the first or earliest issue or part."@en,
        "Met une manifestation en relation avec un titre propre figurant sur une livraison ou partie ultérieure d’une monographie en plusieurs parties ou d’une publication en série et qui diffère de celui figurant sur la première ou la plus ancienne livraison ou partie."@fr .

<http://rdaregistry.info/Elements/m/P30130> a rdf:Property ;
    rdfs:label "has earlier title proper"@en,
        "a pour titre propre antérieur"@fr,
        "har föregående huvudtitel"@sv ;
    rdakit:instructionNumber "2.3.7" ;
    rdakit:toolkitDefinition "A title proper appearing on an earlier iteration of an integrating resource that differs from that on the current iteration."@en,
        "Un título propiamente dicho que aparece en una iteración anterior de un recurso integrable que difiere del que aparece en la iteración actual."@es,
        "Titre propre figurant sur une itération antérieure d’une ressource intégratrice et qui diffère du titre de l’itération en cours."@fr ;
    rdakit:toolkitLabel "earlier title proper"@en,
        "título propiamente dicho anterior"@es,
        "titre propre antérieur"@fr,
        "föregående huvudtitel"@sv ;
    reg:hasUnconstrained <http://rdaregistry.info/Elements/u/P60358> ;
    reg:lexicalAlias <http://rdaregistry.info/Elements/m/earlierTitleProper.en> ;
    reg:name "earlierTitleProper"@en ;
    reg:status <http://metadataregistry.org/uri/RegStatus/1001> ;
    rdfs:domain <http://rdaregistry.info/Elements/c/C10007> ;
    rdfs:isDefinedBy <http://rdaregistry.info/Elements/m/> ;
    rdfs:subPropertyOf <http://rdaregistry.info/Elements/m/P30156> ;
    skos:definition "Relates a manifestation to a title proper appearing on an earlier iteration of an integrating resource that differs from that on the current iteration."@en,
        "Met une manifestation en relation avec un titre propre figurant sur une itération antérieure d’une ressource intégratrice et qui diffère du titre de l’itération en cours."@fr .

<http://rdaregistry.info/Elements/m/P30132> a rdf:Property ;
    rdfs:label "has designation of named revision of edition"@en,
        "a pour indication d’une révision nommée d’une édition"@fr,
        "har påföljande upplagebeteckning"@sv ;
    rdakit:instructionNumber "2.5.6" ;
    rdakit:toolkitDefinition "A word, character, or group of words or characters, identifying a particular revision of a named edition."@en,
        "Una palabra, carácter, o un grupo de palabras y/o caracteres, que identifican una revisión particular de una revisión mencionada de una edición."@es,
        "Mot, caractère ou groupe de mots et/ou caractères identifiant une révision particulière d’une édition nommée."@fr ;
    rdakit:toolkitLabel "designation of named revision of edition"@en,
        "designación de una revisión mencionada de una edición"@es,
        "indication d’une révision nommée d’une édition"@fr,
        "påföljande upplagebeteckning"@sv ;
    reg:hasUnconstrained <http://rdaregistry.info/Elements/u/P60364> ;
    reg:lexicalAlias <http://rdaregistry.info/Elements/m/designationOfNamedRevisionOfEdition.en> ;
    reg:name "designationOfNamedRevisionOfEdition"@en ;
    reg:status <http://metadataregistry.org/uri/RegStatus/1001> ;
    rdfs:domain <http://rdaregistry.info/Elements/c/C10007> ;
    rdfs:isDefinedBy <http://rdaregistry.info/Elements/m/> ;
    skos:definition "Relates a manifestation to a word, character, or group of words or characters, identifying a particular revision of a named edition."@en,
        "Met une manifestation en relation avec un mot, un caractère ou un groupe de mots et/ou caractères identifiant une révision particulière d’une édition nommée."@fr .

<http://rdaregistry.info/Elements/m/P30133> a rdf:Property ;
    rdfs:label "has designation of edition"@en,
        "a pour indication de l’édition"@fr,
        "har upplagebeteckning"@sv ;
    rdakit:instructionNumber "2.5.2" ;
    rdakit:toolkitDefinition "A word, character, or group of words or characters, identifying an edition to which a manifestation belongs."@en,
        "Una palabra, carácter, o un grupo de palabras y/o caracteres, que identifican la edición a la que pertenece un recurso"@es,
        "Mot, caractère ou groupe de mots et/ou caractères identifiant l’édition à laquelle appartient la ressource."@fr ;
    rdakit:toolkitLabel "designation of edition"@en,
        "designación de edición"@es,
        "indication de l’édition"@fr,
        "upplagebeteckning"@sv ;
    reg:hasUnconstrained <http://rdaregistry.info/Elements/u/P60365> ;
    reg:lexicalAlias <http://rdaregistry.info/Elements/m/designationOfEdition.en> ;
    reg:name "designationOfEdition"@en ;
    reg:status <http://metadataregistry.org/uri/RegStatus/1001> ;
    rdfs:domain <http://rdaregistry.info/Elements/c/C10007> ;
    rdfs:isDefinedBy <http://rdaregistry.info/Elements/m/> ;
    skos:definition "Relates a manifestation to a word, character, or group of words or characters, identifying an edition to which a manifestation belongs."@en,
        "Met une manifestation en relation avec un mot, un caractère ou un groupe de mots et/ou caractères identifiant l’édition à laquelle appartient la ressource."@fr .

<http://rdaregistry.info/Elements/m/P30135> a rdf:Property ;
    rdfs:label "has work manifested"@en,
        "a pour œuvre manifestée"@fr,
        "har manifesterat verk"@sv ;
    rdakit:instructionNumber "17.8" ;
    rdakit:toolkitDefinition "A work embodied in a manifestation."@en,
        "Una obra materializada en una manifestación."@es,
        "L’œuvre matérialisée dans une manifestation."@fr ;
    rdakit:toolkitLabel "work manifested"@en,
        "obra manifestada"@es,
        "œuvre manifestée"@fr,
        "manifesterat verk"@sv ;
    reg:hasSubproperty <http://rdaregistry.info/Elements/m/object/P30135> ;
    reg:lexicalAlias <http://rdaregistry.info/Elements/m/workManifested.en> ;
    reg:name "workManifested"@en ;
    reg:status <http://metadataregistry.org/uri/RegStatus/1001> ;
    rdfs:domain <http://rdaregistry.info/Elements/c/C10007> ;
    rdfs:isDefinedBy <http://rdaregistry.info/Elements/m/> ;
    skos:definition "Relates a manifestation to a work embodied in a manifestation."@en,
        "Met une manifestation en relation avec l’œuvre matérialisée dans une manifestation."@fr .

<http://rdaregistry.info/Elements/m/P30139> a rdf:Property ;
    rdfs:label "has expression manifested"@en,
        "a pour expression manifestée"@fr,
        "har manifesterat uttryck"@sv ;
    rdakit:instructionNumber "17.10" ;
    rdakit:toolkitDefinition "An expression embodied in a manifestation."@en,
        "Una expresión materializada en una manifestación."@es,
        "Expression matérialisée dans une manifestation."@fr ;
    rdakit:toolkitLabel "expression manifested"@en,
        "expresión manifestada"@es,
        "expression manifestée"@fr,
        "manifesterat uttryck"@sv ;
    reg:hasSubproperty <http://rdaregistry.info/Elements/m/object/P30139> ;
    reg:lexicalAlias <http://rdaregistry.info/Elements/m/expressionManifested.en> ;
    reg:name "expressionManifested"@en ;
    reg:status <http://metadataregistry.org/uri/RegStatus/1001> ;
    rdfs:domain <http://rdaregistry.info/Elements/c/C10007> ;
    rdfs:isDefinedBy <http://rdaregistry.info/Elements/m/> ;
    skos:definition "Relates a manifestation to an expression embodied in a manifestation."@en,
        "Met une manifestation en relation avec une expression matérialisée dans une manifestation."@fr .

<http://rdaregistry.info/Elements/m/P30141> a rdf:Property ;
    rdfs:label "has contact information"@en,
        "a pour coordonnées"@fr,
        "har kontaktinformation"@sv ;
    rdakit:instructionNumber "4.3" ;
    rdakit:toolkitDefinition "A name, address, etc., of an organization, etc., from which a manifestation may be obtained."@en,
        "Información sobre la organización, etc., de la cual se puede obtener un recurso."@es,
        "Renseignements sur une organisation, etc. auprès de laquelle une ressource peut être obtenue."@fr ;
    rdakit:toolkitLabel "contact information"@en,
        "información de contacto"@es,
        "coordonnées"@fr,
        "kontaktinformation"@sv ;
    reg:hasUnconstrained <http://rdaregistry.info/Elements/u/P60490> ;
    reg:lexicalAlias <http://rdaregistry.info/Elements/m/contactInformation.en> ;
    reg:name "contactInformation"@en ;
    reg:status <http://metadataregistry.org/uri/RegStatus/1001> ;
    rdfs:domain <http://rdaregistry.info/Elements/c/C10007> ;
    rdfs:isDefinedBy <http://rdaregistry.info/Elements/m/> ;
    skos:definition "Relates a manifestation to a name, address, etc., of an organization, etc., from which a manifestation may be obtained."@en,
        "Met une manifestation en relation avec des renseignements sur une organisation, etc. auprès de laquelle une ressource peut être obtenue."@fr ;
    skos:scopeNote "Contact information includes a name, address, etc. of the publisher, distributor, etc. of a published manifestation, or of the archival repository that holds the manifestation."@en .

<http://rdaregistry.info/Elements/m/P30143> a rdf:Property ;
    rdfs:label "has other title information of series"@en,
        "a pour complément du titre de collection"@fr,
        "har övrig titelinformation för serie"@sv ;
    rdakit:instructionNumber "2.12.4" ;
    rdakit:toolkitDefinition "A word, character, or group of words or characters that appears in conjunction with, and is subordinate to, a title proper of a series."@en,
        "Información que aparece en conjunción con el título propiamente dicho de una serie y está subordinada a él."@es,
        "Information reliée et subordonnée au titre propre d’une collection."@fr ;
    rdakit:toolkitLabel "other title information of series"@en,
        "información complementaria del título de la serie"@es,
        "complément du titre de collection"@fr,
        "övrig titelinformation för serie"@sv ;
    reg:hasUnconstrained <http://rdaregistry.info/Elements/u/P60494> ;
    reg:lexicalAlias <http://rdaregistry.info/Elements/m/otherTitleInformationOfSeries.en> ;
    reg:name "otherTitleInformationOfSeries"@en ;
    reg:status <http://metadataregistry.org/uri/RegStatus/1001> ;
    rdfs:domain <http://rdaregistry.info/Elements/c/C10007> ;
    rdfs:isDefinedBy <http://rdaregistry.info/Elements/m/> ;
    skos:definition "Relates a manifestation to a word, character, or group of words or characters that appears in conjunction with, and is subordinate to, a title proper of a series."@en,
        "Met une manifestation en relation avec une information reliée et subordonnée au titre propre d’une collection."@fr .

<http://rdaregistry.info/Elements/m/P30144> a rdf:Property ;
    rdfs:label "has other title information of subseries"@en,
        "a pour complément du titre de sous-collection"@fr,
        "har övrig titelinformation för underserie"@sv ;
    rdakit:instructionNumber "2.12.12" ;
    rdakit:toolkitDefinition "A word, character, or group of words or characters that appears in conjunction with, and is subordinate to, a title proper of a subseries."@en,
        "Información que aparece en conjunción con el título propiamente dicho de una subserie y está subordinada a él."@es,
        "Information reliée et subordonnée au titre propre d’une sous-collection."@fr ;
    rdakit:toolkitLabel "other title information of subseries"@en,
        "información complementaria del título de la subserie"@es,
        "complément du titre de sous-collection"@fr,
        "övrig titelinformation för underserie"@sv ;
    reg:hasUnconstrained <http://rdaregistry.info/Elements/u/P60495> ;
    reg:lexicalAlias <http://rdaregistry.info/Elements/m/otherTitleInformationOfSubseries.en> ;
    reg:name "otherTitleInformationOfSubseries"@en ;
    reg:status <http://metadataregistry.org/uri/RegStatus/1001> ;
    rdfs:domain <http://rdaregistry.info/Elements/c/C10007> ;
    rdfs:isDefinedBy <http://rdaregistry.info/Elements/m/> ;
    skos:definition "Relates a manifestation to a word, character, or group of words or characters that appears in conjunction with, and is subordinate to, a title proper of a subseries."@en,
        "Met une manifestation en relation avec une information reliée et subordonnée au titre propre d’une sous-collection."@fr .

<http://rdaregistry.info/Elements/m/P30145> a rdf:Property ;
    rdfs:label "has restriction on access to manifestation"@en,
        "a pour restrictions d’accès"@fr,
        "har åtkomstrestriktioner"@sv ;
    rdakit:instructionNumber "4.4" ;
    rdakit:toolkitDefinition "A limitation placed on access to a manifestation."@en,
        "Limitaciones establecidas para el acceso a un recurso."@es,
        "Limitations imposées sur l’accès à une ressource."@fr ;
    rdakit:toolkitLabel "restriction on access to manifestation"@en,
        "restricciones de acceso"@es,
        "restrictions d’accès"@fr,
        "åtkomstrestriktioner"@sv ;
    reg:hasUnconstrained <http://rdaregistry.info/Elements/u/P60496> ;
    reg:lexicalAlias <http://rdaregistry.info/Elements/m/restrictionOnAccessToManifestation.en> ;
    reg:name "restrictionOnAccessToManifestation"@en ;
    reg:status <http://metadataregistry.org/uri/RegStatus/1001> ;
    rdfs:domain <http://rdaregistry.info/Elements/c/C10007> ;
    rdfs:isDefinedBy <http://rdaregistry.info/Elements/m/> ;
    skos:definition "Relates a manifestation to a limitation placed on access to a manifestation."@en,
        "Met une manifestation en relation avec des limitations imposées sur l’accès à une ressource."@fr .

<http://rdaregistry.info/Elements/m/P30146> a rdf:Property ;
    rdfs:label "has restriction on use of manifestation"@en,
        "a pour restrictions d’usage"@fr,
        "har användningsrestriktioner"@sv ;
    rdakit:instructionNumber "4.5" ;
    rdakit:toolkitDefinition "A limitation placed on reproduction, publication, exhibition, etc., of a manifestation."@en,
        "Limitaciones establecidas sobre los usos, tales como reproducción, publicación, exhibición, etc."@es,
        "Limitations imposées sur des usages tels que la reproduction, la publication, l’exposition, etc."@fr ;
    rdakit:toolkitLabel "restriction on use of manifestation"@en,
        "restricciones sobre el uso"@es,
        "restrictions d’usage"@fr,
        "användningsrestriktioner"@sv ;
    reg:hasUnconstrained <http://rdaregistry.info/Elements/u/P60497> ;
    reg:lexicalAlias <http://rdaregistry.info/Elements/m/restrictionOnUseOfManifestation.en> ;
    reg:name "restrictionOnUseOfManifestation"@en ;
    reg:status <http://metadataregistry.org/uri/RegStatus/1001> ;
    rdfs:domain <http://rdaregistry.info/Elements/c/C10007> ;
    rdfs:isDefinedBy <http://rdaregistry.info/Elements/m/> ;
    skos:definition "Relates a manifestation to a limitation placed on reproduction, publication, exhibition, etc., of a manifestation."@en,
        "Met une manifestation en relation avec des limitations imposées sur des usages tels que la reproduction, la publication, l’exposition, etc."@fr .

<http://rdaregistry.info/Elements/m/P30152> a rdf:Property ;
    rdfs:label "has parallel other title information of series"@en,
        "a pour complément du titre parallèle d’une collection"@fr,
        "har parallell övrig titelinformation för serie"@sv ;
    rdakit:instructionNumber "2.12.5" ;
    rdakit:toolkitDefinition "An other title information of a series in a language or script that differs from that recorded in an other title information of series element."@en,
        "Información sobre el título de una serie en una lengua y/o escritura que difiere de la registrada en el elemento información complementaria del título de la serie."@es,
        "Complément du titre d’une collection dans une langue et/ou une écriture différentes de celles enregistrées dans l’élément Complément du titre d’une collection."@fr ;
    rdakit:toolkitLabel "parallel other title information of series"@en,
        "información complementaria paralela del título de la serie"@es,
        "complément du titre parallèle d’une collection"@fr,
        "parallell övrig titelinformation för serie"@sv ;
    reg:hasUnconstrained <http://rdaregistry.info/Elements/u/P60508> ;
    reg:lexicalAlias <http://rdaregistry.info/Elements/m/parallelOtherTitleInformationOfSeries.en> ;
    reg:name "parallelOtherTitleInformationOfSeries"@en ;
    reg:status <http://metadataregistry.org/uri/RegStatus/1001> ;
    rdfs:domain <http://rdaregistry.info/Elements/c/C10007> ;
    rdfs:isDefinedBy <http://rdaregistry.info/Elements/m/> ;
    skos:definition "Relates a manifestation to an other title information of a series in a language or script that differs from that recorded in an other title information of series element."@en,
        "Met une manifestation en relation avec un complément du titre d’une collection dans une langue et/ou une écriture différentes de celles enregistrées dans l’élément Complément du titre d’une collection."@fr .

<http://rdaregistry.info/Elements/m/P30153> a rdf:Property ;
    rdfs:label "has parallel other title information of subseries"@en,
        "a pour complément du titre parallèle d’une sous-collection"@fr,
        "har parallell övrig titelinformation för underserie"@sv ;
    rdakit:instructionNumber "2.12.13" ;
    rdakit:toolkitDefinition "An other title information of a subseries in a language or script that differs from that recorded in an other title information of subseries element."@en,
        "Información complementaria de una subserie en una lengua y/o escritura que difiere de la registrada en el elemento información complementaria del título de la subserie."@es,
        "Complément du titre d’une sous-collection dans une langue et/ou une écriture différentes de celles enregistrées dans l’élément Complément du titre d’une sous-collection."@fr ;
    rdakit:toolkitLabel "parallel other title information of subseries"@en,
        "información complementaria paralela del título de la subserie"@es,
        "complément du titre parallèle d’une sous-collection"@fr,
        "parallell övrig titelinformation för underserie"@sv ;
    reg:hasUnconstrained <http://rdaregistry.info/Elements/u/P60509> ;
    reg:lexicalAlias <http://rdaregistry.info/Elements/m/parallelOtherTitleInformationOfSubseries.en> ;
    reg:name "parallelOtherTitleInformationOfSubseries"@en ;
    reg:status <http://metadataregistry.org/uri/RegStatus/1001> ;
    rdfs:domain <http://rdaregistry.info/Elements/c/C10007> ;
    rdfs:isDefinedBy <http://rdaregistry.info/Elements/m/> ;
    skos:definition "Relates a manifestation to an other title information of a subseries in a language or script that differs from that recorded in an other title information of subseries element."@en,
        "Met une manifestation en relation avec un complément du titre d’une sous-collection dans une langue et/ou une écriture différentes de celles enregistrées dans l’élément Complément du titre d’une sous-collection."@fr .

<http://rdaregistry.info/Elements/m/P30154> a rdf:Property ;
    rdfs:label "has uniform resource locator"@en,
        "a pour adresse URL"@fr,
        "har URL"@sv ;
    rdakit:instructionNumber "4.6" ;
    rdakit:toolkitDefinition "An address of an online resource."@en,
        "La dirección de un recurso de acceso remoto."@es,
        "L’adresse d’une ressource accessible en ligne."@fr ;
    rdakit:toolkitLabel "Uniform Resource Locator"@en,
        "Localizador Uniforme de Recurso"@es,
        "adresse URL"@fr,
        "URL"@sv ;
    reg:hasUnconstrained <http://rdaregistry.info/Elements/u/P60511> ;
    reg:lexicalAlias <http://rdaregistry.info/Elements/m/uniformResourceLocator.en> ;
    reg:name "uniformResourceLocator"@en ;
    reg:status <http://metadataregistry.org/uri/RegStatus/1001> ;
    rdfs:domain <http://rdaregistry.info/Elements/c/C10007> ;
    rdfs:isDefinedBy <http://rdaregistry.info/Elements/m/> ;
    skos:altLabel "URL"@en ;
    skos:definition "Relates a manifestation to an address of an online resource."@en,
        "Met une manifestation en relation avec l’adresse d’une ressource accessible en ligne."@fr ;
    skos:scopeNote "A Uniform Resource Locator includes all manifestation identifiers intended to provide online access to a manifestation using a standard Internet browser."@en .

<http://rdaregistry.info/Elements/m/P30155> a rdf:Property ;
    rdfs:label "has layout"@en,
        "a pour disposition"@fr,
        "har layout"@sv ;
    rdakit:instructionNumber "3.11" ;
    rdakit:toolkitDefinition "An arrangement of text, images, tactile notation, etc., in a manifestation."@en,
        "El arreglo del texto, imágenes, notación táctil, etc., en un recurso."@es,
        "L’agencement du texte, des images, etc. dans une ressource."@fr ;
    rdakit:toolkitLabel "layout"@en,
        "presentación"@es,
        "disposition"@fr,
        "layout"@sv ;
    reg:hasUnconstrained <http://rdaregistry.info/Elements/u/P60513> ;
    reg:lexicalAlias <http://rdaregistry.info/Elements/m/layout.en> ;
    reg:name "layout"@en ;
    reg:status <http://metadataregistry.org/uri/RegStatus/1001> ;
    rdfs:domain <http://rdaregistry.info/Elements/c/C10007> ;
    rdfs:isDefinedBy <http://rdaregistry.info/Elements/m/> ;
    skos:definition "Relates a manifestation to an arrangement of text, images, tactile notation, etc., in a manifestation."@en,
        "Met une manifestation en relation avec l’agencement du texte, des images, etc. dans une ressource."@fr .

<http://rdaregistry.info/Elements/m/P30157> a rdf:Property ;
    rdfs:label "has title proper of series"@en,
        "a pour titre propre de la collection"@fr,
        "har huvudtitel till serie"@sv ;
    rdakit:instructionNumber "2.12.2" ;
    rdakit:toolkitDefinition "A name of a series appearing on a manifestation of a part of a series."@en,
        "El nombre principal de la serie (i.e., el título normalmente usado para citar la serie)."@es,
        "Le titre principal d’une collection (c’est-à-dire le titre normalement utilisé pour citer la collection)."@fr ;
    rdakit:toolkitLabel "title proper of series"@en,
        "título propiamente dicho de la serie"@es,
        "titre propre de la collection"@fr,
        "huvudtitel till serie"@sv ;
    reg:hasUnconstrained <http://rdaregistry.info/Elements/u/P60516> ;
    reg:lexicalAlias <http://rdaregistry.info/Elements/m/titleProperOfSeries.en> ;
    reg:name "titleProperOfSeries"@en ;
    reg:status <http://metadataregistry.org/uri/RegStatus/1001> ;
    rdfs:domain <http://rdaregistry.info/Elements/c/C10007> ;
    rdfs:isDefinedBy <http://rdaregistry.info/Elements/m/> ;
    skos:definition "Relates a manifestation to a name of a series appearing on a manifestation of a part of a series."@en,
        "Met une manifestation en relation avec le titre principal d’une collection (c’est-à-dire le titre normalement utilisé pour citer la collection)."@fr .

<http://rdaregistry.info/Elements/m/P30158> a rdf:Property ;
    rdfs:label "has title proper of subseries"@en,
        "a pour titre propre de la sous-collection"@fr,
        "har huvudtitel till underserie"@sv ;
    rdakit:instructionNumber "2.12.10" ;
    rdakit:toolkitDefinition "A name of a series appearing on a manifestation of a part of a subseries."@en,
        "El nombre principal de la subserie (i.e., el título normalmente usado para citar la subserie)."@es,
        "Le titre principal d’une sous-collection (c’est-à-dire le titre normalement utilisé pour citer la sous-collection)."@fr ;
    rdakit:toolkitLabel "title proper of subseries"@en,
        "título propiamente dicho de la subserie"@es,
        "titre propre de la sous-collection"@fr,
        "huvudtitel till underserie"@sv ;
    reg:hasUnconstrained <http://rdaregistry.info/Elements/u/P60517> ;
    reg:lexicalAlias <http://rdaregistry.info/Elements/m/titleProperOfSubseries.en> ;
    reg:name "titleProperOfSubseries"@en ;
    reg:status <http://metadataregistry.org/uri/RegStatus/1001> ;
    rdfs:domain <http://rdaregistry.info/Elements/c/C10007> ;
    rdfs:isDefinedBy <http://rdaregistry.info/Elements/m/> ;
    skos:definition "Relates a manifestation to a name of a series appearing on a manifestation of a part of a subseries."@en,
        "Met une manifestation en relation avec le titre principal d’une sous-collection (c’est-à-dire le titre normalement utilisé pour citer la sous-collection)."@fr .

<http://rdaregistry.info/Elements/m/P30160> a rdf:Property ;
    rdfs:label "has term of availability"@en,
        "a pour modalités d’acquisition"@fr,
        "har anskaffningsvillkor"@sv ;
    rdakit:instructionNumber "4.2" ;
    rdakit:toolkitDefinition "A condition under which the publisher, distributor, etc., will normally supply a manifestation or the price of a manifestation."@en,
        "Las condiciones bajo las cuales el editor, distribuidor, etc., normalmente ofrecerá un recurso o el precio del recurso."@es,
        "Les conditions auxquelles l’éditeur, le diffuseur ou le distributeur, etc. fournit normalement une ressource ou bien le prix d’une ressource."@fr ;
    rdakit:toolkitLabel "term of availability"@en,
        "términos de disponibilidad"@es,
        "modalités d’acquisition"@fr,
        "anskaffningsvillkor"@sv ;
    reg:hasUnconstrained <http://rdaregistry.info/Elements/u/P60521> ;
    reg:lexicalAlias <http://rdaregistry.info/Elements/m/termOfAvailability.en> ;
    reg:name "termOfAvailability"@en ;
    reg:status <http://metadataregistry.org/uri/RegStatus/1001> ;
    rdfs:domain <http://rdaregistry.info/Elements/c/C10007> ;
    rdfs:isDefinedBy <http://rdaregistry.info/Elements/m/> ;
    skos:definition "Relates a manifestation to a condition under which the publisher, distributor, etc., will normally supply a manifestation or the price of a manifestation."@en,
        "Met une manifestation en relation avec les conditions auxquelles l’éditeur, le diffuseur ou le distributeur, etc. fournit normalement une ressource ou bien le prix d’une ressource."@fr .

<http://rdaregistry.info/Elements/m/P30162> a rdf:Property ;
    rdfs:label "has equipment or system requirement"@en,
        "a pour équipement ou système requis"@fr,
        "har utrustning eller systemkrav"@sv ;
    rdakit:instructionNumber "3.20" ;
    rdakit:toolkitDefinition "A system or equipment required for use, playback, etc., of an analog, digital, etc., manifestation."@en,
        "El equipo o sistema requerido para usar, reproducir, etc., un recurso análogo, digital, etc."@es,
        "L’équipement ou le système nécessaire pour l’utilisation, la lecture, etc. d’une ressource analogique, numérique, etc."@fr ;
    rdakit:toolkitLabel "equipment or system requirement"@en,
        "requerimientos de equipo o sistema"@es,
        "équipement ou système requis"@fr,
        "utrustning eller systemkrav"@sv ;
    reg:hasUnconstrained <http://rdaregistry.info/Elements/u/P60528> ;
    reg:lexicalAlias <http://rdaregistry.info/Elements/m/equipmentOrSystemRequirement.en> ;
    reg:name "equipmentOrSystemRequirement"@en ;
    reg:status <http://metadataregistry.org/uri/RegStatus/1001> ;
    rdfs:domain <http://rdaregistry.info/Elements/c/C10007> ;
    rdfs:isDefinedBy <http://rdaregistry.info/Elements/m/> ;
    skos:definition "Relates a manifestation to a system or equipment required for use, playback, etc., of an analog, digital, etc., manifestation."@en,
        "Met une manifestation en relation avec l’équipement ou le système nécessaire pour l’utilisation, la lecture, etc. d’une ressource analogique, numérique, etc."@fr .

<http://rdaregistry.info/Elements/m/P30166> a rdf:Property ;
    rdfs:label "has ISSN of series"@en,
        "a pour ISSN de collection"@fr,
        "har series ISSN"@sv ;
    rdakit:instructionNumber "2.12.8" ;
    rdakit:toolkitDefinition "An identifier assigned to a series by an ISSN registration agency."@en,
        "El identificador asignado a una serie por una agencia de registro del ISSN."@es,
        "L’identifiant attribué à une collection par une agence d’enregistrement de l’ISSN."@fr ;
    rdakit:toolkitLabel "ISSN of series"@en,
        "ISSN de series"@es,
        "ISSN de collection"@fr,
        "series ISSN"@sv ;
    reg:hasUnconstrained <http://rdaregistry.info/Elements/u/P60534> ;
    reg:lexicalAlias <http://rdaregistry.info/Elements/m/issnOfSeries.en> ;
    reg:name "issnOfSeries"@en ;
    reg:status <http://metadataregistry.org/uri/RegStatus/1001> ;
    rdfs:domain <http://rdaregistry.info/Elements/c/C10007> ;
    rdfs:isDefinedBy <http://rdaregistry.info/Elements/m/> ;
    skos:definition "Relates a manifestation to an identifier assigned to a series by an ISSN registration agency."@en,
        "Met une manifestation en relation avec l’identifiant attribué à une collection par une agence d’enregistrement de l’ISSN."@fr .

<http://rdaregistry.info/Elements/m/P30167> a rdf:Property ;
    rdfs:label "has ISSN of subseries"@en,
        "a pour ISSN de sous-collection"@fr,
        "har underseries ISSN"@sv ;
    rdakit:instructionNumber "2.12.16" ;
    rdakit:toolkitDefinition "An identifier assigned to a subseries by an ISSN registration agency."@en,
        "El identificador asignado a una subserie por una agencia de registro del ISSN."@es,
        "L’identifiant attribué à une sous-collection par une agence d’enregistrement de l’ISSN."@fr ;
    rdakit:toolkitLabel "ISSN of subseries"@en,
        "ISSN de la subserie"@es,
        "ISSN de sous-collection"@fr,
        "underseries ISSN"@sv ;
    reg:hasUnconstrained <http://rdaregistry.info/Elements/u/P60535> ;
    reg:lexicalAlias <http://rdaregistry.info/Elements/m/issnOfSubseries.en> ;
    reg:name "issnOfSubseries"@en ;
    reg:status <http://metadataregistry.org/uri/RegStatus/1001> ;
    rdfs:domain <http://rdaregistry.info/Elements/c/C10007> ;
    rdfs:isDefinedBy <http://rdaregistry.info/Elements/m/> ;
    skos:definition "Relates a manifestation to an identifier assigned to a subseries by an ISSN registration agency."@en,
        "Met une manifestation en relation avec l’identifiant attribué à une sous-collection par une agence d’enregistrement de l’ISSN."@fr .

<http://rdaregistry.info/Elements/m/P30168> a rdf:Property ;
    rdfs:label "has frequency"@en,
        "a pour périodicité"@fr,
        "har utgivningsfrekvens"@sv ;
    rdakit:instructionNumber "2.14" ;
    rdakit:toolkitDefinition "An interval at which an issue or part of a serial or an update to an integrating resource is issued."@en,
        "El intervalo en el cual se editan las entregas o partes de una publicación seriada o las actualizaciones de un recurso integrado."@es,
        "Les intervalles de temps suivant lesquels les livraisons ou parties d’une publication en série ou les mises à jour d’une ressource intégratrice sont publiées."@fr ;
    rdakit:toolkitLabel "frequency"@en,
        "frecuencia"@es,
        "périodicité"@fr,
        "utgivningsfrekvens"@sv ;
    reg:hasUnconstrained <http://rdaregistry.info/Elements/u/P60538> ;
    reg:lexicalAlias <http://rdaregistry.info/Elements/m/frequency.en> ;
    reg:name "frequency"@en ;
    reg:status <http://metadataregistry.org/uri/RegStatus/1001> ;
    rdfs:domain <http://rdaregistry.info/Elements/c/C10007> ;
    rdfs:isDefinedBy <http://rdaregistry.info/Elements/m/> ;
    skos:definition "Relates a manifestation to an interval at which an issue or part of a serial or an update to an integrating resource is issued."@en,
        "Met une manifestation en relation avec les intervalles de temps suivant lesquels les livraisons ou parties d’une publication en série ou les mises à jour d’une ressource intégratrice sont publiées."@fr .

<http://rdaregistry.info/Elements/m/P30173> a rdf:Property ;
    rdfs:label "has distributor’s name"@en,
        "a pour nom du diffuseur ou du distributeur"@fr,
        "har distributörsnamn"@sv ;
    rdakit:instructionNumber "2.9.4" ;
    rdakit:toolkitDefinition "A name of an agent responsible for distributing a manifestation in a published form."@en,
        "El nombre de una persona, familia o entidad corporativa responsable de la distribución de un recurso publicado."@es,
        "Le nom d’une personne, famille ou collectivité responsable de la diffusion ou de la distribution d’une ressource sous une forme publiée."@fr ;
    rdakit:toolkitLabel "distributor's name"@en,
        "nombre del distribuidor"@es,
        "nom du diffuseur ou du distributeur"@fr,
        "distributörsnamn"@sv ;
    reg:hasUnconstrained <http://rdaregistry.info/Elements/u/P60544> ;
    reg:lexicalAlias <http://rdaregistry.info/Elements/m/distributorsName.en> ;
    reg:name "distributorsName"@en ;
    reg:status <http://metadataregistry.org/uri/RegStatus/1001> ;
    rdfs:domain <http://rdaregistry.info/Elements/c/C10007> ;
    rdfs:isDefinedBy <http://rdaregistry.info/Elements/m/> ;
    skos:definition "Relates a manifestation to a name of an agent responsible for distributing a manifestation in a published form."@en,
        "Met une manifestation en relation avec le nom d’une personne, famille ou collectivité responsable de la diffusion ou de la distribution d’une ressource sous une forme publiée."@fr .

<http://rdaregistry.info/Elements/m/P30174> a rdf:Property ;
    rdfs:label "has producer’s name"@en,
        "a pour nom du producteur"@fr,
        "har producentnamn"@sv ;
    rdakit:instructionNumber "2.7.4" ;
    rdakit:toolkitDefinition "A name of an agent responsible for inscribing, fabricating, constructing, etc., a manifestation in an unpublished form."@en,
        "El nombre de una persona, familia o entidad corporativa responsable de la inscripción, fabricación, construcción, etc., de un recurso en un formato inédito."@es,
        "Le nom d’une personne, famille ou collectivité responsable de la scription, de la fabrication, de la construction, etc. d’une ressource sous une forme non publiée."@fr ;
    rdakit:toolkitLabel "producer's name"@en,
        "nombre del productor"@es,
        "nom du producteur"@fr,
        "producentnamn"@sv ;
    reg:hasUnconstrained <http://rdaregistry.info/Elements/u/P60545> ;
    reg:lexicalAlias <http://rdaregistry.info/Elements/m/producersName.en> ;
    reg:name "producersName"@en ;
    reg:status <http://metadataregistry.org/uri/RegStatus/1001> ;
    rdfs:domain <http://rdaregistry.info/Elements/c/C10007> ;
    rdfs:isDefinedBy <http://rdaregistry.info/Elements/m/> ;
    skos:definition "Relates a manifestation to a name of an agent responsible for inscribing, fabricating, constructing, etc., a manifestation in an unpublished form."@en,
        "Met une manifestation en relation avec le nom d’une personne, famille ou collectivité responsable de la scription, de la fabrication, de la construction, etc. d’une ressource sous une forme non publiée."@fr .

<http://rdaregistry.info/Elements/m/P30175> a rdf:Property ;
    rdfs:label "has manufacturer’s name"@en,
        "a pour nom du fabricant"@fr,
        "har tillverkarnamn"@sv ;
    rdakit:instructionNumber "2.10.4" ;
    rdakit:toolkitDefinition "A name of an agent responsible for printing, duplicating, casting, etc., a manifestation in a published form."@en,
        "El nombre de una persona, familia o entidad corporativa responsable por la impresión, duplicación prensado etc., de un recurso publicado."@es,
        "Le nom d’une personne, famille ou collectivité responsable de l’impression, de la reproduction, du moulage, etc. d’une ressource sous une forme publiée."@fr ;
    rdakit:toolkitLabel "manufacturer's name"@en,
        "nombre del fabricante"@es,
        "nom du fabricant"@fr,
        "tillverkarnamn"@sv ;
    reg:hasUnconstrained <http://rdaregistry.info/Elements/u/P60546> ;
    reg:lexicalAlias <http://rdaregistry.info/Elements/m/manufacturersName.en> ;
    reg:name "manufacturersName"@en ;
    reg:status <http://metadataregistry.org/uri/RegStatus/1001> ;
    rdfs:domain <http://rdaregistry.info/Elements/c/C10007> ;
    rdfs:isDefinedBy <http://rdaregistry.info/Elements/m/> ;
    skos:definition "Relates a manifestation to a name of an agent responsible for printing, duplicating, casting, etc., a manifestation in a published form."@en,
        "Met une manifestation en relation avec le nom d’une personne, famille ou collectivité responsable de l’impression, de la reproduction, du moulage, etc. d’une ressource sous une forme publiée."@fr .

<http://rdaregistry.info/Elements/m/P30176> a rdf:Property ;
    rdfs:label "has publisher’s name"@en,
        "a pour nom de l’éditeur"@fr,
        "har utgivarnamn"@sv ;
    rdakit:instructionNumber "2.8.4" ;
    rdakit:toolkitDefinition "A name of an agent responsible for publishing, releasing, or issuing a manifestation."@en,
        "El nombre de una persona, familia o entidad corporativa responsable por la publicación, entrega o emisión de un recurso."@es,
        "Le nom d’une personne, famille ou collectivité responsable de la publication, de la mise à disposition ou de l’édition d’une ressource."@fr ;
    rdakit:toolkitLabel "publisher's name"@en,
        "nombre del editor"@es,
        "nom de l’éditeur"@fr,
        "utgivarnamn"@sv ;
    reg:hasUnconstrained <http://rdaregistry.info/Elements/u/P60547> ;
    reg:lexicalAlias <http://rdaregistry.info/Elements/m/publishersName.en> ;
    reg:name "publishersName"@en ;
    reg:status <http://metadataregistry.org/uri/RegStatus/1001> ;
    rdfs:domain <http://rdaregistry.info/Elements/c/C10007> ;
    rdfs:isDefinedBy <http://rdaregistry.info/Elements/m/> ;
    skos:definition "Relates a manifestation to a name of an agent responsible for publishing, releasing, or issuing a manifestation."@en,
        "Met une manifestation en relation avec le nom d’une personne, famille ou collectivité responsable de la publication, de la mise à disposition ou de l’édition d’une ressource."@fr .

<http://rdaregistry.info/Elements/m/P30186> a rdf:Property ;
    rdfs:label "has mount"@en,
        "a pour monture"@fr,
        "har montering"@sv ;
    rdakit:instructionNumber "3.8" ;
    rdakit:toolkitDefinition "A physical material used for the support or backing to which the base material of a manifestation has been attached."@en,
        "El material físico usado como soporte en el cual se sostiene el material base de un recurso."@es,
        "Le matériau physique utilisé pour le support ou le renforcement, sur lequel le matériau de base d’une ressource est fixé."@fr ;
    rdakit:toolkitLabel "mount"@en,
        "montura"@es,
        "monture"@fr,
        "montering"@sv ;
    reg:hasUnconstrained <http://rdaregistry.info/Elements/u/P60554> ;
    reg:lexicalAlias <http://rdaregistry.info/Elements/m/mount.en> ;
    reg:name "mount"@en ;
    reg:status <http://metadataregistry.org/uri/RegStatus/1001> ;
    rdfs:domain <http://rdaregistry.info/Elements/c/C10007> ;
    rdfs:isDefinedBy <http://rdaregistry.info/Elements/m/> ;
    skos:definition "Relates a manifestation to a physical material used for the support or backing to which the base material of a manifestation has been attached."@en,
        "Met une manifestation en relation avec le matériau physique utilisé pour le support ou le renforcement, sur lequel le matériau de base d’une ressource est fixé."@fr .

<http://rdaregistry.info/Elements/m/P30196> a rdf:Property ;
    rdfs:label "has polarity"@en,
        "a pour polarité"@fr,
        "har polaritet"@sv ;
    rdakit:instructionNumber "3.14" ;
    rdakit:toolkitDefinition "A relationship of the colours and tones in an image to the colours and tones of the object reproduced."@en,
        "La relación de los colores y tonos en una imagen con los colores y tonos del objeto reproducido (por ej., positiva, negativa)."@es,
        "La relation des couleurs et des tons d’une image avec les couleurs et les tons de l’objet reproduit (par exemple, positif, négatif)."@fr ;
    rdakit:toolkitLabel "polarity"@en,
        "polaridad"@es,
        "polarité"@fr,
        "polaritet"@sv ;
    reg:hasUnconstrained <http://rdaregistry.info/Elements/u/P60573> ;
    reg:lexicalAlias <http://rdaregistry.info/Elements/m/polarity.en> ;
    reg:name "polarity"@en ;
    reg:status <http://metadataregistry.org/uri/RegStatus/1001> ;
    rdfs:domain <http://rdaregistry.info/Elements/c/C10007> ;
    rdfs:isDefinedBy <http://rdaregistry.info/Elements/m/> ;
    skos:definition "Relates a manifestation to a relationship of the colours and tones in an image to the colours and tones of the object reproduced."@en,
        "Met une manifestation en relation avec la relation des couleurs et des tons d’une image avec les couleurs et les tons de l’objet reproduit (par exemple, positif, négatif)."@fr .

<http://rdaregistry.info/Elements/m/P30197> a rdf:Property ;
    rdfs:label "has bibliographic format"@en,
        "a pour format du livre"@fr,
        "har bokformat"@sv ;
    rdakit:instructionNumber "3.12" ;
    rdakit:toolkitDefinition "A proportional relationship between a whole sheet in a printed or manuscript resource, and the individual leaves that result if that sheet is left full, cut, or folded."@en,
        "El resultado del plegado de una hoja impresa para formar un conjunto de hojas (por ej., una hoja doblada una vez para formar un folio, dos veces para formar un cuarto, tres veces para formar un octavo)."@es,
        "Le résultat du pliage d’une feuille imprimée pour former un cahier de feuillets (par exemple, une feuille pliée une fois pour former un in-folio, pliée deux fois pour former un in-quarto, pliée trois fois pour former un in-octavo, etc.)."@fr ;
    rdakit:toolkitLabel "bibliographic format"@en,
        "formato libro"@es,
        "format du livre"@fr,
        "bokformat"@sv ;
    reg:hasUnconstrained <http://rdaregistry.info/Elements/u/P60578> ;
    reg:lexicalAlias <http://rdaregistry.info/Elements/m/bibliographicFormat.en> ;
    reg:name "bibliographicFormat"@en ;
    reg:status <http://metadataregistry.org/uri/RegStatus/1001> ;
    rdfs:domain <http://rdaregistry.info/Elements/c/C10007> ;
    rdfs:isDefinedBy <http://rdaregistry.info/Elements/m/> ;
    skos:definition "Relates a manifestation to a proportional relationship between a whole sheet in a printed or manuscript resource, and the individual leaves that result if that sheet is left full, cut, or folded."@en,
        "Met une manifestation en relation avec le résultat du pliage d’une feuille imprimée pour former un cahier de feuillets (par exemple, une feuille pliée une fois pour former un in-folio, pliée deux fois pour former un in-quarto, pliée trois fois pour former un in-octavo, etc.)."@fr .

<http://rdaregistry.info/Elements/m/P30198> a rdf:Property ;
    rdfs:label "has reduction ratio"@en,
        "a pour facteur de réduction"@fr,
        "har förminskningsgrad"@sv ;
    rdakit:instructionNumber "3.15" ;
    rdakit:toolkitDefinition "A numerical ratio of the size of a micro-image in relation to the original from which it was produced."@en,
        "El tamaño de una microimagen en relación con el original del cual se produjo."@es,
        "La taille d’une micro-image par rapport à celle de l’original à partir duquel elle a été produite."@fr ;
    rdakit:toolkitLabel "reduction ratio"@en,
        "escala de reducción"@es,
        "facteur de réduction"@fr,
        "förminskningsgrad"@sv ;
    reg:hasUnconstrained <http://rdaregistry.info/Elements/u/P60581> ;
    reg:lexicalAlias <http://rdaregistry.info/Elements/m/reductionRatio.en> ;
    reg:name "reductionRatio"@en ;
    reg:status <http://metadataregistry.org/uri/RegStatus/1001> ;
    rdfs:domain <http://rdaregistry.info/Elements/c/C10007> ;
    rdfs:isDefinedBy <http://rdaregistry.info/Elements/m/> ;
    skos:definition "Relates a manifestation to a numerical ratio of the size of a micro-image in relation to the original from which it was produced."@en,
        "Met une manifestation en relation avec la taille d’une micro-image par rapport à celle de l’original à partir duquel elle a été produite."@fr .

<http://rdaregistry.info/Elements/m/P30199> a rdf:Property ;
    rdfs:label "has font size"@en,
        "a pour taille de la police de caractères"@fr,
        "har teckenstorlek"@sv ;
    rdakit:instructionNumber "3.13" ;
    rdakit:toolkitDefinition "A size of the type used to represent the characters and symbols in a manifestation."@en,
        "El tamaño del tipo utilizado para representar los caracteres y símbolos en un recurso."@es,
        "La taille des caractères utilisés pour représenter les signes et les symboles dans une ressource."@fr ;
    rdakit:toolkitLabel "font size"@en,
        "tamaño de la fuente"@es,
        "taille de la police de caractères"@fr,
        "teckenstorlek"@sv ;
    reg:hasUnconstrained <http://rdaregistry.info/Elements/u/P60582> ;
    reg:lexicalAlias <http://rdaregistry.info/Elements/m/fontSize.en> ;
    reg:name "fontSize"@en ;
    reg:status <http://metadataregistry.org/uri/RegStatus/1001> ;
    rdfs:domain <http://rdaregistry.info/Elements/c/C10007> ;
    rdfs:isDefinedBy <http://rdaregistry.info/Elements/m/> ;
    skos:definition "Relates a manifestation to a size of the type used to represent the characters and symbols in a manifestation."@en,
        "Met une manifestation en relation avec la taille des caractères utilisés pour représenter les signes et les symboles dans une ressource."@fr .

<http://rdaregistry.info/Elements/m/P30204> a rdf:Property ;
    rdfs:label "has parallel title proper of series"@en,
        "a pour titre propre parallèle de la collection"@fr,
        "har parallel title proper of series"@sv ;
    rdakit:instructionNumber "2.12.3" ;
    rdakit:toolkitDefinition "A title proper of a series in another language or script."@en,
        "El título propiamente dicho de una serie en otra lengua y/o escritura."@es,
        "Le titre propre d’une collection dans une autre langue et/ou écriture."@fr ;
    rdakit:toolkitLabel "parallel title proper of series"@en,
        "título paralelo propiamente dicho de la serie"@es,
        "titre propre parallèle de la collection"@fr,
        "parallell huvudtitel till serie"@sv ;
    reg:hasUnconstrained <http://rdaregistry.info/Elements/u/P60590> ;
    reg:lexicalAlias <http://rdaregistry.info/Elements/m/parallelTitleProperOfSeries.en> ;
    reg:name "parallelTitleProperOfSeries"@en ;
    reg:status <http://metadataregistry.org/uri/RegStatus/1001> ;
    rdfs:domain <http://rdaregistry.info/Elements/c/C10007> ;
    rdfs:isDefinedBy <http://rdaregistry.info/Elements/m/> ;
    skos:definition "Relates a manifestation to a title proper of a series in another language or script."@en,
        "Met une manifestation en relation avec le titre propre d’une collection dans une autre langue et/ou écriture."@fr .

<http://rdaregistry.info/Elements/m/P30205> a rdf:Property ;
    rdfs:label "has parallel title proper of subseries"@en,
        "a pour titre propre parallèle de la sous-collection"@fr,
        "har parallell huvudtitel till underserie"@sv ;
    rdakit:instructionNumber "2.12.11" ;
    rdakit:toolkitDefinition "A title proper of a subseries in another language or script."@en,
        "El título propiamente dicho de una subserie en otra lengua y/o escritura."@es,
        "Le titre propre d’une sous-collection dans une autre langue et/ou écriture."@fr ;
    rdakit:toolkitLabel "parallel title proper of subseries"@en,
        "título paralelo propiamente dicho de la subserie"@es,
        "titre propre parallèle de la sous-collection"@fr,
        "parallell huvudtitel till underserie"@sv ;
    reg:hasUnconstrained <http://rdaregistry.info/Elements/u/P60591> ;
    reg:lexicalAlias <http://rdaregistry.info/Elements/m/parallelTitleProperOfSubseries.en> ;
    reg:name "parallelTitleProperOfSubseries"@en ;
    reg:status <http://metadataregistry.org/uri/RegStatus/1001> ;
    rdfs:domain <http://rdaregistry.info/Elements/c/C10007> ;
    rdfs:isDefinedBy <http://rdaregistry.info/Elements/m/> ;
    skos:definition "Relates a manifestation to a title proper of a subseries in another language or script."@en,
        "Met une manifestation en relation avec le titre propre d’une sous-collection dans une autre langue et/ou écriture."@fr .

<http://rdaregistry.info/Elements/m/P30207> a rdf:Property ;
    reg:status <http://metadataregistry.org/uri/RegStatus/1008> ;
    rdfs:isDefinedBy <http://rdaregistry.info/Elements/m/> .

<http://rdaregistry.info/Elements/m/P30208> a rdf:Property ;
    rdfs:label "has base material"@en,
        "a pour matériau de base"@fr,
        "har bärande material"@sv ;
    rdakit:instructionNumber "3.6" ;
    rdakit:toolkitDefinition "An underlying physical material of a manifestation."@en,
        "Material físico que sostiene el recurso."@es,
        "Le matériau physique sous-jacent d’une ressource."@fr ;
    rdakit:toolkitLabel "base material"@en,
        "material base"@es,
        "matériau de base"@fr,
        "bärande material"@sv ;
    reg:hasUnconstrained <http://rdaregistry.info/Elements/u/P60596> ;
    reg:lexicalAlias <http://rdaregistry.info/Elements/m/baseMaterial.en> ;
    reg:name "baseMaterial"@en ;
    reg:status <http://metadataregistry.org/uri/RegStatus/1001> ;
    rdfs:domain <http://rdaregistry.info/Elements/c/C10007> ;
    rdfs:isDefinedBy <http://rdaregistry.info/Elements/m/> ;
    skos:definition "Relates a manifestation to an underlying physical material of a manifestation."@en,
        "Met une manifestation en relation avec le matériau physique sous-jacent d’une ressource."@fr .

<http://rdaregistry.info/Elements/m/P30211> a rdf:Property ;
    reg:status <http://metadataregistry.org/uri/RegStatus/1008> ;
    rdfs:isDefinedBy <http://rdaregistry.info/Elements/m/> .

<http://rdaregistry.info/Elements/m/P30217> a rdf:Property ;
    rdfs:label "has details of base material"@en,
        "har detaljerad information om bärande matieral"@sv ;
    rdakit:instructionNumber "3.6.1.4" ;
    rdakit:toolkitDefinition "Details of an underlying physical material of a manifestation."@en,
        "Detalles del material físico que sostiene el recurso."@es ;
    rdakit:toolkitLabel "details of base material"@en,
        "detalles del material de base"@es,
        "detaljerad information om bärande matieral"@sv ;
    reg:hasUnconstrained <http://rdaregistry.info/Elements/u/P60768> ;
    reg:lexicalAlias <http://rdaregistry.info/Elements/m/detailsOfBaseMaterial.en> ;
    reg:name "detailsOfBaseMaterial"@en ;
    reg:status <http://metadataregistry.org/uri/RegStatus/1001> ;
    rdfs:domain <http://rdaregistry.info/Elements/c/C10007> ;
    rdfs:isDefinedBy <http://rdaregistry.info/Elements/m/> ;
    skos:definition "Relates a manifestation to details of an underlying physical material of a manifestation."@en .

<http://rdaregistry.info/Elements/m/P30218> a rdf:Property ;
    rdfs:label "has details of bibliographic format"@en,
        "har detaljerad information om bokformat"@sv ;
    rdakit:instructionNumber "3.12.1.4" ;
    rdakit:toolkitDefinition "Details of a proportional relationship between a whole sheet in a printed or manuscript resource, and the individual leaves that result if that sheet is left full, cut, or folded."@en,
        "Detalles del resultado del plegado de una hoja impresa para formar un conjunto de hojas (por ej., una hoja doblada una vez para formar un folio, dos veces para formar un cuarto, tres veces para formar un octavo)."@es ;
    rdakit:toolkitLabel "details of bibliographic format"@en,
        "detalles del formato libro"@es,
        "detaljerad information om bokformat"@sv ;
    reg:hasUnconstrained <http://rdaregistry.info/Elements/u/P60769> ;
    reg:lexicalAlias <http://rdaregistry.info/Elements/m/detailsOfBibliographicFormat.en> ;
    reg:name "detailsOfBibliographicFormat"@en ;
    reg:status <http://metadataregistry.org/uri/RegStatus/1001> ;
    rdfs:domain <http://rdaregistry.info/Elements/c/C10007> ;
    rdfs:isDefinedBy <http://rdaregistry.info/Elements/m/> ;
    skos:definition "Relates a manifestation to details of a proportional relationship between a whole sheet in a printed or manuscript resource, and the individual leaves that result if that sheet is left full, cut, or folded."@en .

<http://rdaregistry.info/Elements/m/P30226> a rdf:Property ;
    rdfs:label "has details of font size"@en,
        "har detaljerad information om teckenstorlek"@sv ;
    rdakit:instructionNumber "3.13.1.4" ;
    rdakit:toolkitDefinition "Details of a size of the type used to represent the characters and symbols in a manifestation."@en,
        "Detalles del tamaño del tipo utilizado para representar los caracteres y símbolos en un recurso."@es ;
    rdakit:toolkitLabel "details of font size"@en,
        "detalles del tamaño de la fuente"@es,
        "detaljerad information om teckenstorlek"@sv ;
    reg:hasUnconstrained <http://rdaregistry.info/Elements/u/P60777> ;
    reg:lexicalAlias <http://rdaregistry.info/Elements/m/detailsOfFontSize.en> ;
    reg:name "detailsOfFontSize"@en ;
    reg:status <http://metadataregistry.org/uri/RegStatus/1001> ;
    rdfs:domain <http://rdaregistry.info/Elements/c/C10007> ;
    rdfs:isDefinedBy <http://rdaregistry.info/Elements/m/> ;
    skos:definition "Relates a manifestation to details of a size of the type used to represent the characters and symbols in a manifestation."@en .

<http://rdaregistry.info/Elements/m/P30227> a rdf:Property ;
    rdakit:instructionNumber "3.10.2.4" ;
    rdakit:toolkitDefinition "Detalles de la relación entre un soporte de audio original y el soporte de una reproducción hecha del original (por ej., cinta maestra de duplicación, una impresión de prueba)."@es ;
    rdakit:toolkitLabel "details of generation of audio recording"@en,
        "detalles de la generación de la grabación sonora"@es ;
    reg:hasUnconstrained <http://rdaregistry.info/Elements/u/P60778> ;
    reg:lexicalAlias <http://rdaregistry.info/Elements/m/detailsOfGenerationOfAudioRecording.en> ;
    reg:name "detailsOfGenerationOfAudioRecording"@en ;
    reg:status <http://metadataregistry.org/uri/RegStatus/1008> ;
    rdfs:domain <http://rdaregistry.info/Elements/c/C10007> ;
    rdfs:isDefinedBy <http://rdaregistry.info/Elements/m/> .

<http://rdaregistry.info/Elements/m/P30228> a rdf:Property ;
    rdakit:instructionNumber "3.10.3.4" ;
    rdakit:toolkitDefinition "Detalles de la relación entre el soporte original de un recurso digital y el soporte de una reproducción del original (por ej., máster derivado)."@es ;
    rdakit:toolkitLabel "details of generation of digital resource"@en,
        "detalles de la generaión del recurso digital"@es ;
    reg:hasUnconstrained <http://rdaregistry.info/Elements/u/P60779> ;
    reg:lexicalAlias <http://rdaregistry.info/Elements/m/detailsOfGenerationOfDigitalResource.en> ;
    reg:name "detailsOfGenerationOfDigitalResource"@en ;
    reg:status <http://metadataregistry.org/uri/RegStatus/1008> ;
    rdfs:domain <http://rdaregistry.info/Elements/c/C10007> ;
    rdfs:isDefinedBy <http://rdaregistry.info/Elements/m/> .

<http://rdaregistry.info/Elements/m/P30229> a rdf:Property ;
    rdakit:instructionNumber "3.10.4.4" ;
    rdakit:toolkitDefinition "Detalles de la relación entre el soporte original de una microforma y el soporte de una reproducción hecha del original (por ej., un máster de impresión)."@es ;
    rdakit:toolkitLabel "details of generation of microform"@en,
        "detalles de la generación de la microforma"@es ;
    reg:hasUnconstrained <http://rdaregistry.info/Elements/u/P60780> ;
    reg:lexicalAlias <http://rdaregistry.info/Elements/m/detailsOfGenerationOfMicroform.en> ;
    reg:name "detailsOfGenerationOfMicroform"@en ;
    reg:status <http://metadataregistry.org/uri/RegStatus/1008> ;
    rdfs:domain <http://rdaregistry.info/Elements/c/C10007> ;
    rdfs:isDefinedBy <http://rdaregistry.info/Elements/m/> .

<http://rdaregistry.info/Elements/m/P30230> a rdf:Property ;
    rdakit:instructionNumber "3.10.5.4" ;
    rdakit:toolkitDefinition "Detalles de la relación entre un soporte original de una película cinematográfica como recurso y el soporte de la reproducción hecha del original (por ej., impreso de referencia)."@es ;
    rdakit:toolkitLabel "details of generation of motion picture film"@en,
        "detalles de la generación de la película cinematográfica"@es ;
    reg:hasUnconstrained <http://rdaregistry.info/Elements/u/P60781> ;
    reg:lexicalAlias <http://rdaregistry.info/Elements/m/detailsOfGenerationOfMotionPictureFilm.en> ;
    reg:name "detailsOfGenerationOfMotionPictureFilm"@en ;
    reg:status <http://metadataregistry.org/uri/RegStatus/1008> ;
    rdfs:domain <http://rdaregistry.info/Elements/c/C10007> ;
    rdfs:isDefinedBy <http://rdaregistry.info/Elements/m/> .

<http://rdaregistry.info/Elements/m/P30231> a rdf:Property ;
    rdakit:instructionNumber "3.10.6.4" ;
    rdakit:toolkitDefinition "Detalles de la relación entre un soporte original de un recurso en videocinta y el soporte de una reproducción hecha del original (por ej., copia de exhibición)."@es ;
    rdakit:toolkitLabel "details of generation of videotape"@en,
        "detalles de la generación de la videocinta"@es ;
    reg:hasUnconstrained <http://rdaregistry.info/Elements/u/P60782> ;
    reg:lexicalAlias <http://rdaregistry.info/Elements/m/detailsOfGenerationOfVideotape.en> ;
    reg:name "detailsOfGenerationOfVideotape"@en ;
    reg:status <http://metadataregistry.org/uri/RegStatus/1008> ;
    rdfs:domain <http://rdaregistry.info/Elements/c/C10007> ;
    rdfs:isDefinedBy <http://rdaregistry.info/Elements/m/> .

<http://rdaregistry.info/Elements/m/P30233> a rdf:Property ;
    rdfs:label "has details of layout"@en,
        "har detaljerad information om layout"@sv ;
    rdakit:instructionNumber "3.11.1.4" ;
    rdakit:toolkitDefinition "Details of an arrangement of text, images, tactile notation, etc., in a manifestation."@en,
        "Detalles del arreglo del texto, imágenes, notación táctil, etc., en un recurso."@es ;
    rdakit:toolkitLabel "details of layout"@en,
        "detalles de la presentación"@es,
        "detaljerad information om layout"@sv ;
    reg:hasUnconstrained <http://rdaregistry.info/Elements/u/P60784> ;
    reg:lexicalAlias <http://rdaregistry.info/Elements/m/detailsOfLayout.en> ;
    reg:name "detailsOfLayout"@en ;
    reg:status <http://metadataregistry.org/uri/RegStatus/1001> ;
    rdfs:domain <http://rdaregistry.info/Elements/c/C10007> ;
    rdfs:isDefinedBy <http://rdaregistry.info/Elements/m/> ;
    skos:definition "Relates a manifestation to details of an arrangement of text, images, tactile notation, etc., in a manifestation."@en .

<http://rdaregistry.info/Elements/m/P30234> a rdf:Property ;
    rdfs:label "has details of mount"@en,
        "har detaljerad information om montering"@sv ;
    rdakit:instructionNumber "3.8.1.4" ;
    rdakit:toolkitDefinition "Details of a physical material used for the support or backing to which the base material of a manifestation has been attached."@en,
        "Detalles del material físico usado como soporte en el cual se sostiene el material base de un recurso."@es ;
    rdakit:toolkitLabel "details of mount"@en,
        "detalles de la montura"@es,
        "detaljerad information om montering"@sv ;
    reg:hasUnconstrained <http://rdaregistry.info/Elements/u/P60785> ;
    reg:lexicalAlias <http://rdaregistry.info/Elements/m/detailsOfMount.en> ;
    reg:name "detailsOfMount"@en ;
    reg:status <http://metadataregistry.org/uri/RegStatus/1001> ;
    rdfs:domain <http://rdaregistry.info/Elements/c/C10007> ;
    rdfs:isDefinedBy <http://rdaregistry.info/Elements/m/> ;
    skos:definition "Relates a manifestation to details of a physical material used for the support or backing to which the base material of a manifestation has been attached."@en .

<http://rdaregistry.info/Elements/m/P30235> a rdf:Property ;
    rdfs:label "has details of playing speed"@en,
        "har details of playing speed"@sv ;
    rdakit:instructionNumber "3.16.4.4" ;
    rdakit:toolkitDefinition "Details of a speed at which an audio carrier must be operated to produce the sound intended."@en,
        "Detalles de la velocidad a la cual un soporte de audio debe ser operado para producir el sonido esperado."@es ;
    rdakit:toolkitLabel "details of playing speed"@en,
        "detalles de la velocidad de reproducción"@es,
        "detaljerad information om uppspelningshastighet"@sv ;
    reg:hasUnconstrained <http://rdaregistry.info/Elements/u/P60786> ;
    reg:lexicalAlias <http://rdaregistry.info/Elements/m/detailsOfPlayingSpeed.en> ;
    reg:name "detailsOfPlayingSpeed"@en ;
    reg:status <http://metadataregistry.org/uri/RegStatus/1001> ;
    rdfs:domain <http://rdaregistry.info/Elements/c/C10007> ;
    rdfs:isDefinedBy <http://rdaregistry.info/Elements/m/> ;
    skos:definition "Relates a manifestation to details of a speed at which an audio carrier must be operated to produce the sound intended."@en .

<http://rdaregistry.info/Elements/m/P30236> a rdf:Property ;
    rdfs:label "has details of polarity"@en,
        "har detaljerad information om polaritet"@sv ;
    rdakit:instructionNumber "3.14.1.4" ;
    rdakit:toolkitDefinition "Details of a relationship of the colours and tones in an image to the colours and tones of the object reproduced."@en,
        "Detalles de la relación de los colores y tonos en una imagen con los colores y tonos del objeto reproducido (por ej., positiva, negativa)."@es ;
    rdakit:toolkitLabel "details of polarity"@en,
        "detalles de la polaridad"@es,
        "detaljerad information om polaritet"@sv ;
    reg:hasUnconstrained <http://rdaregistry.info/Elements/u/P60787> ;
    reg:lexicalAlias <http://rdaregistry.info/Elements/m/detailsOfPolarity.en> ;
    reg:name "detailsOfPolarity"@en ;
    reg:status <http://metadataregistry.org/uri/RegStatus/1001> ;
    rdfs:domain <http://rdaregistry.info/Elements/c/C10007> ;
    rdfs:isDefinedBy <http://rdaregistry.info/Elements/m/> ;
    skos:definition "Relates a manifestation to details of a relationship of the colours and tones in an image to the colours and tones of the object reproduced."@en .

<http://rdaregistry.info/Elements/m/P30237> a rdf:Property ;
    rdfs:label "has details of presentation format"@en,
        "har detaljerad information om filmprojektionssystem"@sv ;
    rdakit:instructionNumber "3.17.2.4" ;
    rdakit:toolkitDefinition "Details of a format used in the production of a projected image."@en,
        "Detalles del formato utilizado en la producción de una imagen proyectada (por ej., Cinerama, IMAX)."@es ;
    rdakit:toolkitLabel "details of presentation format"@en,
        "detalles del formato de presentación"@es,
        "detaljerad information om filmprojektionssystem"@sv ;
    reg:hasUnconstrained <http://rdaregistry.info/Elements/u/P60788> ;
    reg:lexicalAlias <http://rdaregistry.info/Elements/m/detailsOfPresentationFormat.en> ;
    reg:name "detailsOfPresentationFormat"@en ;
    reg:status <http://metadataregistry.org/uri/RegStatus/1001> ;
    rdfs:domain <http://rdaregistry.info/Elements/c/C10007> ;
    rdfs:isDefinedBy <http://rdaregistry.info/Elements/m/> ;
    skos:definition "Relates a manifestation to details of a format used in the production of a projected image."@en .

<http://rdaregistry.info/Elements/m/P30238> a rdf:Property ;
    rdfs:label "has details of production method"@en,
        "har detaljerad information om produktionsmetod"@sv ;
    rdakit:instructionNumber "3.9.1.4" ;
    rdakit:toolkitDefinition "Details of a process used to produce a manifestation."@en,
        "Detalles del proceso utilizado para producir un recurso."@es ;
    rdakit:toolkitLabel "details of production method"@en,
        "detalles del método de producción"@es,
        "detaljerad information om produktionsmetod"@sv ;
    reg:hasUnconstrained <http://rdaregistry.info/Elements/u/P60789> ;
    reg:lexicalAlias <http://rdaregistry.info/Elements/m/detailsOfProductionMethod.en> ;
    reg:name "detailsOfProductionMethod"@en ;
    reg:status <http://metadataregistry.org/uri/RegStatus/1001> ;
    rdfs:domain <http://rdaregistry.info/Elements/c/C10007> ;
    rdfs:isDefinedBy <http://rdaregistry.info/Elements/m/> ;
    skos:definition "Relates a manifestation to details of a process used to produce a manifestation."@en .

<http://rdaregistry.info/Elements/m/P30239> a rdf:Property ;
    reg:hasUnconstrained <http://rdaregistry.info/Elements/u/P60790> ;
    reg:lexicalAlias <http://rdaregistry.info/Elements/m/detailsOfProductionMethodForManuscript.en> ;
    reg:name "detailsOfProductionMethodForManuscript"@en ;
    reg:status <http://metadataregistry.org/uri/RegStatus/1008> ;
    rdfs:domain <http://rdaregistry.info/Elements/c/C10007> ;
    rdfs:isDefinedBy <http://rdaregistry.info/Elements/m/> .

<http://rdaregistry.info/Elements/m/P30240> a rdf:Property ;
    rdakit:instructionNumber "3.9.3.4" ;
    rdakit:toolkitDefinition "Detalles del proceso utilizado para producir un recurso táctil (por ej., repujado, termoformado)."@es ;
    rdakit:toolkitLabel "detalles del método de producción de un recurso táctil"@es ;
    reg:hasUnconstrained <http://rdaregistry.info/Elements/u/P60791> ;
    reg:lexicalAlias <http://rdaregistry.info/Elements/m/detailsOfProductionMethodForTactileResource.en> ;
    reg:name "detailsOfProductionMethodForTactileResource"@en ;
    reg:status <http://metadataregistry.org/uri/RegStatus/1008> ;
    rdfs:domain <http://rdaregistry.info/Elements/c/C10007> ;
    rdfs:isDefinedBy <http://rdaregistry.info/Elements/m/> .

<http://rdaregistry.info/Elements/m/P30244> a rdf:Property ;
    rdfs:label "has details of reduction ratio designation"@en,
        "har detaljerad information om förminskningsgrad"@sv ;
    rdakit:instructionNumber "3.15.1.5.1.4" ;
    rdakit:toolkitDefinition "Details of a designation of the size of a micro-image to the original from which it was produced."@en,
        "Detalles del tamaño de una microimagen en relación con el original del cual se produjo."@es ;
    rdakit:toolkitLabel "details of reduction ratio designation"@en,
        "detalles de la escala de reducción"@es,
        "detaljerad information om förminskningsgrad"@sv ;
    reg:hasUnconstrained <http://rdaregistry.info/Elements/u/P60795> ;
    reg:lexicalAlias <http://rdaregistry.info/Elements/m/detailsOfReductionRatioDesignation.en> ;
    reg:name "detailsOfReductionRatioDesignation"@en ;
    reg:status <http://metadataregistry.org/uri/RegStatus/1001> ;
    rdfs:domain <http://rdaregistry.info/Elements/c/C10007> ;
    rdfs:isDefinedBy <http://rdaregistry.info/Elements/m/> ;
    skos:definition "Relates a manifestation to details of a general designation of the size of a micro-image to the original from which it was produced."@en .

<http://rdaregistry.info/Elements/m/P30252> a rdf:Property ;
    rdfs:label "has details of generation"@en,
        "har detaljerad information om generation"@sv ;
    rdakit:instructionNumber "3.10.1.4" ;
    rdakit:toolkitDefinition "Details of a relationship between an original carrier and a carrier of a reproduction made from an original."@en,
        "Detalles de la relación entre un soporte original y el soporte de una reproducción del original (por ej., una cámara maestra de primera generación, una impresión maestra de segunda generación)."@es ;
    rdakit:toolkitLabel "details of generation"@en,
        "detalles de generación"@es,
        "detaljerad information om generation"@sv ;
    reg:hasUnconstrained <http://rdaregistry.info/Elements/u/P60803> ;
    reg:lexicalAlias <http://rdaregistry.info/Elements/m/detailsOfGeneration.en> ;
    reg:name "detailsOfGeneration"@en ;
    reg:status <http://metadataregistry.org/uri/RegStatus/1001> ;
    rdfs:domain <http://rdaregistry.info/Elements/c/C10007> ;
    rdfs:isDefinedBy <http://rdaregistry.info/Elements/m/> ;
    skos:definition "Relates a manifestation to details of a relationship between an original carrier and a carrier of a reproduction made from an original."@en .

<http://rdaregistry.info/Elements/m/P30261> a rdf:Property ;
    rdfs:label "has cartographic data type"@en ;
    rdakit:instructionNumber "3.19.8.5" ;
    rdakit:toolkitDefinition "A machine-readable representation of geospatial features."@en ;
    rdakit:toolkitLabel "cartographic data type"@en ;
    reg:hasUnconstrained <http://rdaregistry.info/Elements/u/P60875> ;
    reg:lexicalAlias <http://rdaregistry.info/Elements/m/cartographicDataType.en> ;
    reg:name "cartographicDataType"@en ;
    reg:status <http://metadataregistry.org/uri/RegStatus/1001> ;
    rdfs:domain <http://rdaregistry.info/Elements/c/C10007> ;
    rdfs:isDefinedBy <http://rdaregistry.info/Elements/m/> ;
    skos:definition "Relates a manifestation to a machine-readable representation of geospatial features."@en .

<http://rdaregistry.info/Elements/m/P30262> a rdf:Property ;
    rdfs:label "has details of cartographic data type"@en ;
    rdakit:instructionNumber "3.19.8.5.4" ;
    rdakit:toolkitDefinition "Details of a machine-readable representation of geospatial features."@en ;
    rdakit:toolkitLabel "details of cartographic data type"@en ;
    reg:hasSubproperty <http://rdaregistry.info/Elements/m/object/P30262> ;
    reg:hasUnconstrained <http://rdaregistry.info/Elements/u/P60876> ;
    reg:lexicalAlias <http://rdaregistry.info/Elements/m/detailsOfCartographicDataType.en> ;
    reg:name "detailsOfCartographicDataType"@en ;
    reg:status <http://metadataregistry.org/uri/RegStatus/1001> ;
    rdfs:domain <http://rdaregistry.info/Elements/c/C10007> ;
    rdfs:isDefinedBy <http://rdaregistry.info/Elements/m/> ;
    skos:definition "Relates a manifestation to details of a machine-readable representation of geospatial features."@en .

<http://rdaregistry.info/Elements/m/P30263> a rdf:Property ;
    rdfs:label "has reduction ratio designation"@en ;
    rdakit:instructionNumber "3.15.1.5" ;
    rdakit:toolkitDefinition "A general designation of the size of a micro-image in relation to the original from which it was produced."@en ;
    rdakit:toolkitLabel "reduction ratio designation"@en ;
    reg:hasSubproperty <http://rdaregistry.info/Elements/m/object/P30263> ;
    reg:hasUnconstrained <http://rdaregistry.info/Elements/u/P60877> ;
    reg:lexicalAlias <http://rdaregistry.info/Elements/m/reductionRatioDesignation.en> ;
    reg:name "reductionRatioDesignation"@en ;
    reg:status <http://metadataregistry.org/uri/RegStatus/1001> ;
    rdfs:domain <http://rdaregistry.info/Elements/c/C10007> ;
    rdfs:isDefinedBy <http://rdaregistry.info/Elements/m/> ;
    skos:definition "Relates a manifestation to a general designation of the size of a micro-image in relation to the original from which it was produced."@en .

<http://rdaregistry.info/Elements/m/P30275> a rdf:Property ;
    rdfs:label "has details of regional encoding"@en ;
    rdakit:instructionNumber "3.19.6.4" ;
    rdakit:toolkitDefinition "Details of a designation for one or more regions of the world for which a videodisc or video game carrier has been encoded, indicating that playback is restricted to a device configured to decode it."@en ;
    rdakit:toolkitLabel "details of regional encoding"@en ;
    reg:hasUnconstrained <http://rdaregistry.info/Elements/u/P60904> ;
    reg:lexicalAlias <http://rdaregistry.info/Elements/m/detailsOfRegionalEncoding.en> ;
    reg:name "detailsOfRegionalEncoding"@en ;
    reg:status <http://metadataregistry.org/uri/RegStatus/1001> ;
    rdfs:domain <http://rdaregistry.info/Elements/c/C10007> ;
    rdfs:isDefinedBy <http://rdaregistry.info/Elements/m/> ;
    rdfs:subPropertyOf <http://rdaregistry.info/Elements/m/P30221> ;
    skos:definition "Relates a manifestation to details of a designation for one or more regions of the world for which a videodisc or video game carrier has been encoded, indicating that playback is restricted to a device configured to decode it."@en .

<http://rdaregistry.info/Elements/m/P30006> a rdf:Property ;
    rdfs:label "has regional encoding"@en,
        "a pour code de région"@fr,
        "har regionkod"@sv ;
    rdakit:instructionNumber "3.19.6" ;
    rdakit:toolkitDefinition "A designation for one or more regions of the world for which a videodisc or video game carrier has been encoded, indicating that playback is restricted to a device configured to decode it."@en,
        "Un código que identifica la región del mundo para la cual se codificó el videodisco DVD, para prevenir que el disco se use en un reproductor vendido en una región diferente."@es,
        "Code identifiant la région du monde pour laquelle un vidéodisque a été encodé et empêchant le disque d’être lu sur un lecteur vendu dans une région différente."@fr ;
    rdakit:toolkitLabel "regional encoding"@en,
        "codificación regional"@es,
        "code de région"@fr,
        "regionkod"@sv ;
    reg:hasUnconstrained <http://rdaregistry.info/Elements/u/P60059> ;
    reg:lexicalAlias <http://rdaregistry.info/Elements/m/regionalEncoding.en> ;
    reg:name "regionalEncoding"@en ;
    reg:status <http://metadataregistry.org/uri/RegStatus/1001> ;
    rdfs:domain <http://rdaregistry.info/Elements/c/C10007> ;
    rdfs:isDefinedBy <http://rdaregistry.info/Elements/m/> ;
    rdfs:subPropertyOf <http://rdaregistry.info/Elements/m/P30124> ;
    skos:definition "Relates a manifestation to a designation for one or more regions of the world for which a videodisc or video game carrier has been encoded, indicating that playback is restricted to a device configured to decode it."@en,
        "Met une manifestation en relation avec un code identifiant la région du monde pour laquelle un vidéodisque a été encodé et empêchant le disque d’être lu sur un lecteur vendu dans une région différente."@fr .

<http://rdaregistry.info/Elements/m/P30016> a rdf:Property ;
    rdfs:label "has electronic reproduction (manifestation)"@en,
        "a pour reproduction électronique (manifestation)"@fr ;
    rdakit:instructionNumber "24.5" ;
    rdakit:toolkitDefinition "A manifestation in a digital format that is the result of the transfer of a manifestation in an analog format."@en,
        "Una manifestación en un formato digital que es el resultado de la transferencia de una manifestación en un formato análogo."@es,
        "Manifestation en format numérique qui est le résultat du transfert d’une manifestation sur support analogique."@fr ;
    rdakit:toolkitLabel "electronic reproduction (manifestation)"@en,
        "reproducción electrónica (manifestación)"@es,
        "reproduction électronique (manifestation)"@fr ;
    reg:hasSubproperty <http://rdaregistry.info/Elements/m/object/P30016> ;
    reg:hasUnconstrained <http://rdaregistry.info/Elements/u/P60083> ;
    reg:lexicalAlias <http://rdaregistry.info/Elements/m/electronicReproductionManifestation.en> ;
    reg:name "electronicReproductionManifestation"@en ;
    reg:status <http://metadataregistry.org/uri/RegStatus/1001> ;
    rdfs:domain <http://rdaregistry.info/Elements/c/C10007> ;
    rdfs:isDefinedBy <http://rdaregistry.info/Elements/m/> ;
    rdfs:subPropertyOf <http://rdaregistry.info/Elements/m/P30039> ;
    skos:definition "Relates a manifestation to a manifestation in a digital format that is the result of the transfer of a manifestation in an analog format."@en,
        "Met une manifestation en relation avec une manifestation en format numérique qui est le résultat du transfert d’une manifestation sur support analogique."@fr .

<http://rdaregistry.info/Elements/m/P30018> a rdf:Property ;
    rdfs:label "has file type"@en,
        "a pour type de fichier"@fr,
        "har filtyp"@sv ;
    rdakit:instructionNumber "3.19.2" ;
    rdakit:toolkitDefinition "A general type of data content encoded in a computer file."@en,
        "Un tipo general de contenido de datos codificado en un archivo de computadora."@es,
        "Type général de contenu des données encodées dans un fichier informatique."@fr ;
    rdakit:toolkitLabel "file type"@en,
        "tipo de archivo"@es,
        "type de fichier"@fr,
        "filtyp"@sv ;
    reg:hasUnconstrained <http://rdaregistry.info/Elements/u/P60093> ;
    reg:lexicalAlias <http://rdaregistry.info/Elements/m/fileType.en> ;
    reg:name "fileType"@en ;
    reg:status <http://metadataregistry.org/uri/RegStatus/1001> ;
    rdfs:domain <http://rdaregistry.info/Elements/c/C10007> ;
    rdfs:isDefinedBy <http://rdaregistry.info/Elements/m/> ;
    rdfs:subPropertyOf <http://rdaregistry.info/Elements/m/P30124> ;
    skos:definition "Relates a manifestation to a general type of data content encoded in a computer file."@en,
        "Met une manifestation en relation avec un type général de contenu des données encodées dans un fichier informatique."@fr .

<http://rdaregistry.info/Elements/m/P30019> a rdf:Property ;
    rdfs:label "is facsimile contained in"@en,
        "est le fac-similé contenu dans (manifestation)"@fr ;
    rdakit:instructionNumber "24.5" ;
    rdakit:toolkitDefinition "A larger manifestation of which a part is a discrete component that exactly reproduces another manifestation embodying the same expression of a work."@en,
        "Una manifestación mayor de la cual una parte es un componente independiente que reproduce exactamente otra manifestación que materializa la misma expresión de una obra."@es,
        "Manifestation plus vaste dont une partie est une composante distincte qui reproduit exactement une autre manifestation matérialisant la même expression d’une œuvre."@fr ;
    rdakit:toolkitLabel "facsimile contained in"@en,
        "facsímil contenido en (manifestación)"@es,
        "fac-similé contenu dans (manifestation)"@fr ;
    reg:hasSubproperty <http://rdaregistry.info/Elements/m/object/P30019> ;
    reg:hasUnconstrained <http://rdaregistry.info/Elements/u/P60100> ;
    reg:lexicalAlias <http://rdaregistry.info/Elements/m/facsimileContainedIn.en> ;
    reg:name "facsimileContainedIn"@en ;
    reg:status <http://metadataregistry.org/uri/RegStatus/1001> ;
    rdfs:domain <http://rdaregistry.info/Elements/c/C10007> ;
    rdfs:isDefinedBy <http://rdaregistry.info/Elements/m/> ;
    rdfs:subPropertyOf <http://rdaregistry.info/Elements/m/P30020> ;
    skos:definition "Relates a manifestation to a larger manifestation of which a part is a discrete component that exactly reproduces another manifestation embodying the same expression of a work."@en,
        "Met une manifestation en relation avec une manifestation plus vaste dont une partie est une composante distincte qui reproduit exactement une autre manifestation matérialisant la même expression d’une œuvre."@fr .

<http://rdaregistry.info/Elements/m/P30021> a rdf:Property ;
    rdfs:label "has preservation facsimile (manifestation)"@en,
        "a pour fac-similé de conservation"@fr ;
    rdakit:instructionNumber "24.5" ;
    rdakit:toolkitDefinition "A manifestation that consists of an exact reproduction on preservation-quality media, such as acid-free permanent or archival paper."@en,
        "Una manifestación que consiste en una reproducción exacta en un medio con calidad de preservación, tal como papel libre de ácido o papel de archivo."@es,
        "Manifestation qui consiste en une reproduction exacte sur un support de qualité conservation, tel qu’un papier permanent sans acide ou un papier d’archivage."@fr ;
    rdakit:toolkitLabel "preservation facsimile (manifestation)"@en,
        "facsímil de preservación (manifestación)"@es,
        "fac-similé de conservation"@fr ;
    reg:hasSubproperty <http://rdaregistry.info/Elements/m/object/P30021> ;
    reg:hasUnconstrained <http://rdaregistry.info/Elements/u/P60179> ;
    reg:lexicalAlias <http://rdaregistry.info/Elements/m/preservationFacsimileManifestation.en> ;
    reg:name "preservationFacsimileManifestation"@en ;
    reg:status <http://metadataregistry.org/uri/RegStatus/1001> ;
    rdfs:domain <http://rdaregistry.info/Elements/c/C10007> ;
    rdfs:isDefinedBy <http://rdaregistry.info/Elements/m/> ;
    rdfs:subPropertyOf <http://rdaregistry.info/Elements/m/P30031> ;
    skos:definition "Relates a manifestation to a manifestation that consists of an exact reproduction on preservation-quality media, such as acid-free permanent or archival paper."@en,
        "Met une manifestation en relation avec une manifestation qui consiste en une reproduction exacte sur un support de qualité conservation, tel qu’un papier permanent sans acide ou un papier d’archivage."@fr .

<http://rdaregistry.info/Elements/m/P30022> a rdf:Property ;
    rdfs:label "is insert"@en,
        "est l’encart"@fr ;
    rdakit:instructionNumber "24.5" ;
    rdakit:toolkitDefinition "A manifestation consisting of separately issued material that is not an integral part of a larger manifestation into which it has been inserted."@en,
        "Una manifestación que consiste en material publicado separadamente, que no es parte integral de la manifestación mayor en la cual se inserta."@es,
        "Manifestation consistant en un document publié séparément qui ne fait pas partie intégrante de la manifestation plus vaste dans laquelle il a été encarté."@fr ;
    rdakit:toolkitLabel "insert"@en,
        "inserto"@es,
        "encart"@fr ;
    reg:hasSubproperty <http://rdaregistry.info/Elements/m/object/P30022> ;
    reg:hasUnconstrained <http://rdaregistry.info/Elements/u/P60183> ;
    reg:lexicalAlias <http://rdaregistry.info/Elements/m/insert.en> ;
    reg:name "insert"@en ;
    reg:status <http://metadataregistry.org/uri/RegStatus/1001> ;
    rdfs:domain <http://rdaregistry.info/Elements/c/C10007> ;
    rdfs:isDefinedBy <http://rdaregistry.info/Elements/m/> ;
    rdfs:subPropertyOf <http://rdaregistry.info/Elements/m/P30033> ;
    skos:definition "Relates a manifestation to a manifestation consisting of separately issued material that is not an integral part of a larger manifestation into which it has been inserted."@en,
        "Met une manifestation en relation avec une manifestation consistant en un document publié séparément qui ne fait pas partie intégrante de la manifestation plus vaste dans laquelle il a été encarté."@fr .

<http://rdaregistry.info/Elements/m/P30025> a rdf:Property ;
    rdfs:label "is inserted in"@en,
        "est encarté dans"@fr ;
    rdakit:instructionNumber "24.5" ;
    rdakit:toolkitDefinition "A manifestation into which material has been inserted that is not an integral part of the publication."@en,
        "Una manifestación en la cual se ha insertado material que no es parte integral de la publicación."@es,
        "Manifestation dans laquelle un document qui ne fait pas partie intégrante de la publication a été encarté."@fr ;
    rdakit:toolkitLabel "inserted in"@en,
        "insertada en"@es,
        "encarté dans"@fr ;
    reg:hasSubproperty <http://rdaregistry.info/Elements/m/object/P30025> ;
    reg:hasUnconstrained <http://rdaregistry.info/Elements/u/P60194> ;
    reg:lexicalAlias <http://rdaregistry.info/Elements/m/insertedIn.en> ;
    reg:name "insertedIn"@en ;
    reg:status <http://metadataregistry.org/uri/RegStatus/1001> ;
    rdfs:domain <http://rdaregistry.info/Elements/c/C10007> ;
    rdfs:isDefinedBy <http://rdaregistry.info/Elements/m/> ;
    rdfs:subPropertyOf <http://rdaregistry.info/Elements/m/P30020> ;
    skos:definition "Relates a manifestation to a manifestation into which material has been inserted that is not an integral part of the publication."@en,
        "Met une manifestation en relation avec une manifestation dans laquelle un document qui ne fait pas partie intégrante de la publication a été encarté."@fr .

<http://rdaregistry.info/Elements/m/P30026> a rdf:Property ;
    rdfs:label "is also issued as"@en,
        "est publié également comme"@fr ;
    rdakit:instructionNumber "24.5" ;
    rdakit:toolkitDefinition "A manifestation that embodies the same expression of a work in a different format."@en,
        "Una manifestación que materializa la misma expresión de una obra en formato diferente."@es,
        "Manifestation matérialisant la même expression d’une œuvre sur un support différent."@fr ;
    rdakit:toolkitLabel "also issued as"@en,
        "publicada también como"@es,
        "publié également comme"@fr ;
    reg:hasSubproperty <http://rdaregistry.info/Elements/m/object/P30026> ;
    reg:hasUnconstrained <http://rdaregistry.info/Elements/u/P60195> ;
    reg:lexicalAlias <http://rdaregistry.info/Elements/m/alsoIssuedAs.en> ;
    reg:name "alsoIssuedAs"@en ;
    reg:status <http://metadataregistry.org/uri/RegStatus/1001> ;
    rdfs:domain <http://rdaregistry.info/Elements/c/C10007> ;
    rdfs:isDefinedBy <http://rdaregistry.info/Elements/m/> ;
    rdfs:subPropertyOf <http://rdaregistry.info/Elements/m/P30024> ;
    skos:definition "Relates a manifestation to a manifestation that embodies the same expression of a work in a different format."@en,
        "Met une manifestation en relation avec une manifestation matérialisant la même expression d’une œuvre sur un support différent."@fr .

<http://rdaregistry.info/Elements/m/P30028> a rdf:Property ;
    rdfs:label "is mirror site"@en,
        "est le site miroir"@fr ;
    rdakit:instructionNumber "24.5" ;
    rdakit:toolkitDefinition "A manifestation that is an exact copy of a website, used to reduce network traffic or improve the availability of the content of the original site."@en,
        "Una manifestación que es una copia exacta de un sitio web, usada para reducir el tráfico en la red o mejorar la disponibilidad del sitio original."@es,
        "Manifestation qui est une copie exacte d’un site Web, utilisée pour réduire le trafic sur le réseau ou augmenter la disponibilité du contenu du site d’origine."@fr ;
    rdakit:toolkitLabel "mirror site"@en,
        "sitio espejo"@es,
        "site miroir"@fr ;
    reg:hasSubproperty <http://rdaregistry.info/Elements/m/object/P30028> ;
    reg:hasUnconstrained <http://rdaregistry.info/Elements/u/P60197> ;
    reg:lexicalAlias <http://rdaregistry.info/Elements/m/mirrorSite.en> ;
    reg:name "mirrorSite"@en ;
    reg:status <http://metadataregistry.org/uri/RegStatus/1001> ;
    rdfs:domain <http://rdaregistry.info/Elements/c/C10007> ;
    rdfs:isDefinedBy <http://rdaregistry.info/Elements/m/> ;
    rdfs:subPropertyOf <http://rdaregistry.info/Elements/m/P30024> ;
    skos:definition "Relates a manifestation to a manifestation that is an exact copy of a website, used to reduce network traffic or improve the availability of the content of the original site."@en,
        "Met une manifestation en relation avec une manifestation qui est une copie exacte d’un site Web, utilisée pour réduire le trafic sur le réseau ou augmenter la disponibilité du contenu du site d’origine."@fr .

<http://rdaregistry.info/Elements/m/P30029> a rdf:Property ;
    rdfs:label "has digital transfer (manifestation)"@en,
        "a pour transfert numérique (manifestation)"@fr ;
    rdakit:instructionNumber "24.5" ;
    rdakit:toolkitDefinition "A manifestation in a digital format that results from the transfer of a manifestation in another digital format."@en,
        "Una manifestación en formato digital que resulta de la transferencia de una manifestación en otro formato digital."@es,
        "Manifestation en format numérique qui résulte du transfert d’une manifestation dans un format numérique différent."@fr ;
    rdakit:toolkitLabel "digital transfer (manifestation)"@en,
        "transferencia digital (manifestación)"@es,
        "transfert numérique (manifestation)"@fr ;
    reg:hasSubproperty <http://rdaregistry.info/Elements/m/object/P30029> ;
    reg:hasUnconstrained <http://rdaregistry.info/Elements/u/P60200> ;
    reg:lexicalAlias <http://rdaregistry.info/Elements/m/digitalTransferManifestation.en> ;
    reg:name "digitalTransferManifestation"@en ;
    reg:status <http://metadataregistry.org/uri/RegStatus/1001> ;
    rdfs:domain <http://rdaregistry.info/Elements/c/C10007> ;
    rdfs:isDefinedBy <http://rdaregistry.info/Elements/m/> ;
    rdfs:subPropertyOf <http://rdaregistry.info/Elements/m/P30039> ;
    skos:definition "Relates a manifestation to a manifestation in a digital format that results from the transfer of a manifestation in another digital format."@en,
        "Met une manifestation en relation avec une manifestation en format numérique qui résulte du transfert d’une manifestation dans un format numérique différent."@fr .

<http://rdaregistry.info/Elements/m/P30030> a rdf:Property ;
    rdfs:label "is special issue"@en,
        "est le numéro spécial"@fr ;
    rdakit:instructionNumber "24.5" ;
    rdakit:toolkitDefinition "A manifestation that consists of a single issue or a supplementary section of a periodical or newspaper devoted to a special subject, with or without serial numbering."@en,
        "Una manifestación que contiene un número o sección suplementaria de una publicación seriada o periódico dedicada a un tema especial."@es,
        "Manifestation qui consiste en un numéro isolé ou un supplément d’une publication en série ou d’un journal consacré à un sujet spécifique."@fr ;
    rdakit:toolkitLabel "special issue"@en,
        "número especial"@es,
        "numéro spécial"@fr ;
    reg:hasSubproperty <http://rdaregistry.info/Elements/m/object/P30030> ;
    reg:hasUnconstrained <http://rdaregistry.info/Elements/u/P60207> ;
    reg:lexicalAlias <http://rdaregistry.info/Elements/m/specialIssue.en> ;
    reg:name "specialIssue"@en ;
    reg:status <http://metadataregistry.org/uri/RegStatus/1001> ;
    rdfs:domain <http://rdaregistry.info/Elements/c/C10007> ;
    rdfs:isDefinedBy <http://rdaregistry.info/Elements/m/> ;
    rdfs:subPropertyOf <http://rdaregistry.info/Elements/m/P30033> ;
    skos:definition "Relates a manifestation to a manifestation that consists of a single issue or a supplementary section of a periodical or newspaper devoted to a special subject, with or without serial numbering."@en,
        "Met une manifestation en relation avec une manifestation qui consiste en un numéro isolé ou un supplément d’une publication en série ou d’un journal consacré à un sujet spécifique."@fr .

<http://rdaregistry.info/Elements/m/P30036> a rdf:Property ;
    rdfs:label "is on disc with (manifestation)"@en,
        "est sur le disque avec (manifestation)"@fr ;
    rdakit:instructionNumber "24.5" ;
    rdakit:toolkitDefinition "A manifestation that is issued on the same disc with a manifestation being described."@en,
        "Una manifestación que está publicada en el mismo disco que la manifestación que se está describiendo."@es,
        "Manifestation qui est publiée sur le même disque que la manifestation décrite."@fr ;
    rdakit:toolkitLabel "on disc with (manifestation)"@en,
        "en disco con (manifestación)"@es,
        "sur le disque avec (manifestation)"@fr ;
    reg:hasSubproperty <http://rdaregistry.info/Elements/m/object/P30036> ;
    reg:hasUnconstrained <http://rdaregistry.info/Elements/u/P60257> ;
    reg:lexicalAlias <http://rdaregistry.info/Elements/m/onDiscWithManifestation.en> ;
    reg:name "onDiscWithManifestation"@en ;
    reg:status <http://metadataregistry.org/uri/RegStatus/1001> ;
    rdfs:domain <http://rdaregistry.info/Elements/c/C10007> ;
    rdfs:isDefinedBy <http://rdaregistry.info/Elements/m/> ;
    rdfs:subPropertyOf <http://rdaregistry.info/Elements/m/P30035> ;
    skos:definition "Relates a manifestation to a manifestation that is issued on the same disc with a manifestation being described."@en,
        "Met une manifestation en relation avec une manifestation qui est publiée sur le même disque que la manifestation décrite."@fr .

<http://rdaregistry.info/Elements/m/P30037> a rdf:Property ;
    rdfs:label "is filmed with (manifestation)"@en,
        "est filmé avec (manifestation)"@fr ;
    rdakit:instructionNumber "24.5" ;
    rdakit:toolkitDefinition "A manifestation that is issued on the same microform with a manifestation being described."@en,
        "Una manifestación que está publicada en la misma microforma que la manifestación que se está describiendo."@es,
        "Manifestation qui est publiée sur la même microforme que la manifestation décrite."@fr ;
    rdakit:toolkitLabel "filmed with (manifestation)"@en,
        "filmada con (manifestación)"@es,
        "filmé avec (manifestation)"@fr ;
    reg:hasSubproperty <http://rdaregistry.info/Elements/m/object/P30037> ;
    reg:hasUnconstrained <http://rdaregistry.info/Elements/u/P60258> ;
    reg:lexicalAlias <http://rdaregistry.info/Elements/m/filmedWithManifestation.en> ;
    reg:name "filmedWithManifestation"@en ;
    reg:status <http://metadataregistry.org/uri/RegStatus/1001> ;
    rdfs:domain <http://rdaregistry.info/Elements/c/C10007> ;
    rdfs:isDefinedBy <http://rdaregistry.info/Elements/m/> ;
    rdfs:subPropertyOf <http://rdaregistry.info/Elements/m/P30035> ;
    skos:definition "Relates a manifestation to a manifestation that is issued on the same microform with a manifestation being described."@en,
        "Met une manifestation en relation avec une manifestation qui est publiée sur la même microforme que la manifestation décrite."@fr .

<http://rdaregistry.info/Elements/m/P30038> a rdf:Property ;
    rdfs:label "is reprinted as (manifestation)"@en,
        "est réimprimé comme (manifestation)"@fr ;
    rdakit:instructionNumber "24.5" ;
    rdakit:toolkitDefinition "A manifestation that is a reissue of another printed manifestation."@en,
        "Una manifestación que es una reedición de otra manifestación impresa."@es,
        "Manifestation qui est une réédition d’une autre manifestation imprimée."@fr ;
    rdakit:toolkitLabel "reprinted as (manifestation)"@en,
        "reimpreso como (manifestación)"@es,
        "réimprimé comme (manifestation)"@fr ;
    reg:hasSubproperty <http://rdaregistry.info/Elements/m/object/P30038> ;
    reg:hasUnconstrained <http://rdaregistry.info/Elements/u/P60271> ;
    reg:lexicalAlias <http://rdaregistry.info/Elements/m/reprintedAsManifestation.en> ;
    reg:name "reprintedAsManifestation"@en ;
    reg:status <http://metadataregistry.org/uri/RegStatus/1001> ;
    rdfs:domain <http://rdaregistry.info/Elements/c/C10007> ;
    rdfs:isDefinedBy <http://rdaregistry.info/Elements/m/> ;
    rdfs:subPropertyOf <http://rdaregistry.info/Elements/m/P30039> ;
    skos:definition "Relates a manifestation to a manifestation that is a reissue of another printed manifestation."@en,
        "Met une manifestation en relation avec une manifestation qui est une réédition d’une autre manifestation imprimée."@fr .

<http://rdaregistry.info/Elements/m/P30040> a rdf:Property ;
    rdfs:label "is digital transfer of (manifestation)"@en,
        "est le transfert numérique de (manifestation)"@fr ;
    rdakit:instructionNumber "24.5" ;
    rdakit:toolkitDefinition "A manifestation in a digital format that is transferred to another digital format."@en,
        "Una manifestación en un formato digital que se transfiere a otro formato digital."@es,
        "Manifestation en format numérique qui a été transférée dans un format numérique différent."@fr ;
    rdakit:toolkitLabel "digital transfer of (manifestation)"@en,
        "transferencia digital de (manifestación)"@es,
        "transfert numérique de (manifestation)"@fr ;
    reg:hasSubproperty <http://rdaregistry.info/Elements/m/object/P30040> ;
    reg:hasUnconstrained <http://rdaregistry.info/Elements/u/P60287> ;
    reg:lexicalAlias <http://rdaregistry.info/Elements/m/digitalTransferOfManifestation.en> ;
    reg:name "digitalTransferOfManifestation"@en ;
    reg:status <http://metadataregistry.org/uri/RegStatus/1001> ;
    rdfs:domain <http://rdaregistry.info/Elements/c/C10007> ;
    rdfs:isDefinedBy <http://rdaregistry.info/Elements/m/> ;
    rdfs:subPropertyOf <http://rdaregistry.info/Elements/m/P30043> ;
    skos:definition "Relates a manifestation to a manifestation in a digital format that is transferred to another digital format."@en,
        "Met une manifestation en relation avec une manifestation en format numérique qui a été transférée dans un format numérique différent."@fr .

<http://rdaregistry.info/Elements/m/P30045> a rdf:Property ;
    rdfs:label "is preservation facsimile of (manifestation)"@en,
        "est le fac-similé de conservation de (manifestation)"@fr ;
    rdakit:instructionNumber "24.5" ;
    rdakit:toolkitDefinition "A manifestation that is used as the basis for an exact reproduction on preservation-quality media, such as acid-free permanent or archival paper."@en,
        "Una manifestación utilizada como base para una reproducción exacta sobre un medio con calidad de preservación, tal como papel libre de ácido o papel de archivo."@es,
        "Manifestation servant de base à une reproduction exacte sur un support de qualité conservation, tel qu’un papier permanent sans acide ou un papier d’archivage."@fr ;
    rdakit:toolkitLabel "preservation facsimile of (manifestation)"@en,
        "facsímil de preservación de (manifestación)"@es,
        "fac-similé de conservation de (manifestation)"@fr ;
    reg:hasSubproperty <http://rdaregistry.info/Elements/m/object/P30045> ;
    reg:hasUnconstrained <http://rdaregistry.info/Elements/u/P60299> ;
    reg:lexicalAlias <http://rdaregistry.info/Elements/m/preservationFacsimileOfManifestation.en> ;
    reg:name "preservationFacsimileOfManifestation"@en ;
    reg:status <http://metadataregistry.org/uri/RegStatus/1001> ;
    rdfs:domain <http://rdaregistry.info/Elements/c/C10007> ;
    rdfs:isDefinedBy <http://rdaregistry.info/Elements/m/> ;
    rdfs:subPropertyOf <http://rdaregistry.info/Elements/m/P30047> ;
    skos:definition "Relates a manifestation to a manifestation that is used as the basis for an exact reproduction on preservation-quality media, such as acid-free permanent or archival paper."@en,
        "Met une manifestation en relation avec une manifestation servant de base à une reproduction exacte sur un support de qualité conservation, tel qu’un papier permanent sans acide ou un papier d’archivage."@fr .

<http://rdaregistry.info/Elements/m/P30046> a rdf:Property ;
    rdfs:label "is facsimile container of"@en,
        "est le conteneur fac-similé de (manifestation)"@fr ;
    rdakit:instructionNumber "24.5" ;
    rdakit:toolkitDefinition "A manifestation used as the basis for an exact reproduction that is a discrete component of a larger manifestation."@en,
        "Una manifestación utilizada como base para una reproducción exacta que es un componente individual de una entidad mayor."@es,
        "Manifestation servant de base à une reproduction exacte qui est une composante distincte d’une manifestation plus vaste."@fr ;
    rdakit:toolkitLabel "facsimile container of"@en,
        "contiene facsímil de (manifestación)"@es,
        "conteneur fac-similé de (manifestation)"@fr ;
    reg:hasSubproperty <http://rdaregistry.info/Elements/m/object/P30046> ;
    reg:hasUnconstrained <http://rdaregistry.info/Elements/u/P60300> ;
    reg:lexicalAlias <http://rdaregistry.info/Elements/m/facsimileContainerOf.en> ;
    reg:name "facsimileContainerOf"@en ;
    reg:status <http://metadataregistry.org/uri/RegStatus/1001> ;
    rdfs:domain <http://rdaregistry.info/Elements/c/C10007> ;
    rdfs:isDefinedBy <http://rdaregistry.info/Elements/m/> ;
    rdfs:subPropertyOf <http://rdaregistry.info/Elements/m/P30033> ;
    skos:definition "Relates a manifestation to a manifestation used as the basis for an exact reproduction that is a discrete component of a larger manifestation."@en,
        "Met une manifestation en relation avec une manifestation servant de base à une reproduction exacte qui est une composante distincte d’une manifestation plus vaste."@fr .

<http://rdaregistry.info/Elements/m/P30050> a rdf:Property ;
    rdfs:label "has note on issue, part, or iteration used as basis for identification of manifestation"@en,
        "a pour note relative à la livraison, la partie ou l’itération servant de base pour l’identification de la ressource"@fr,
        "har anmärkning om nummer, del eller uppdatering som beskrivningen grundar sig på"@sv ;
    rdakit:instructionNumber "2.17.13" ;
    rdakit:toolkitDefinition "A note identifying an issue or part of a multipart monograph or serial, or an iteration of an integrating resource that has been used as a basis for the identification of a manifestation."@en,
        "Una nota que identifica la entrega o parte de una monografía en varias partes o publicación seriada, o la iteración de un recurso integrado que se ha utilizado como base para la identificación de un recurso."@es,
        "Note identifiant la livraison d’une publication en série ou la partie d’une monographie en plusieurs parties ou bien l’itération d’une ressource intégratrice qui a servi de base pour l’identification d’une ressource."@fr ;
    rdakit:toolkitLabel "note on issue, part, or iteration used as basis for identification of manifestation"@en,
        "nota sobre entrega, parte o iteración usada como base para la identificación del recurso"@es,
        "note relative à la livraison, la partie ou l’itération servant de base pour l’identification de la ressource"@fr,
        "anmärkning om nummer, del eller uppdatering som beskrivningen grundar sig på"@sv ;
    reg:hasUnconstrained <http://rdaregistry.info/Elements/u/P60122> ;
    reg:lexicalAlias <http://rdaregistry.info/Elements/m/noteOnIssuePartOrIterationUsedAsBasisForIdentificationOfManifestation.en> ;
    reg:name "noteOnIssuePartOrIterationUsedAsBasisForIdentificationOfManifestation"@en ;
    reg:status <http://metadataregistry.org/uri/RegStatus/1001> ;
    rdfs:domain <http://rdaregistry.info/Elements/c/C10007> ;
    rdfs:isDefinedBy <http://rdaregistry.info/Elements/m/> ;
    rdfs:subPropertyOf <http://rdaregistry.info/Elements/m/P30137> ;
    skos:definition "Relates a manifestation to a note identifying an issue or part of a multipart monograph or serial, or an iteration of an integrating resource that has been used as a basis for the identification of a manifestation."@en,
        "Met une manifestation en relation avec une note identifiant la livraison d’une publication en série ou la partie d’une monographie en plusieurs parties ou bien l’itération d’une ressource intégratrice qui a servi de base pour l’identification d’une ressource."@fr .

<http://rdaregistry.info/Elements/m/P30051> a rdf:Property ;
    rdfs:label "has note on changes in carrier characteristics"@en,
        "a pour note sur les changements dans les caractéristiques du support matériel"@fr,
        "har anmärkning om förändringar i bäraregenskaper"@sv ;
    rdakit:instructionNumber "3.21.4" ;
    rdakit:toolkitDefinition "A note on changes in the characteristics of the carrier that occur in subsequent issues or parts of a manifestation issued in successive parts or between iterations of an integrating resource."@en,
        "Una nota sobre cambios en las características del soporte que ocurren en entregas o partes subsecuentes del recurso publicado en partes sucesivas o entre iteraciones de un recurso integrado."@es,
        "Note portant sur les changements dans les caractéristiques du support matériel survenant dans les livraisons ou parties ultérieures d’une ressource publiée en parties successives ou bien entre les différentes itérations d’une ressource intégratrice."@fr ;
    rdakit:toolkitLabel "note on changes in carrier characteristics"@en,
        "nota sobre los cambios en las características del soporte"@es,
        "note sur les changements dans les caractéristiques du support matériel"@fr,
        "anmärkning om förändringar i bäraregenskaper"@sv ;
    reg:hasUnconstrained <http://rdaregistry.info/Elements/u/P60124> ;
    reg:lexicalAlias <http://rdaregistry.info/Elements/m/noteOnChangesInCarrierCharacteristics.en> ;
    reg:name "noteOnChangesInCarrierCharacteristics"@en ;
    reg:status <http://metadataregistry.org/uri/RegStatus/1001> ;
    rdfs:domain <http://rdaregistry.info/Elements/c/C10007> ;
    rdfs:isDefinedBy <http://rdaregistry.info/Elements/m/> ;
    rdfs:subPropertyOf <http://rdaregistry.info/Elements/m/P30214> ;
    skos:definition "Relates a manifestation to a note on changes in the characteristics of the carrier that occur in subsequent issues or parts of a manifestation issued in successive parts or between iterations of an integrating resource."@en,
        "Met une manifestation en relation avec une note portant sur les changements dans les caractéristiques du support matériel survenant dans les livraisons ou parties ultérieures d’une ressource publiée en parties successives ou bien entre les différentes itérations d’une ressource intégratrice."@fr .

<http://rdaregistry.info/Elements/m/P30052> a rdf:Property ;
    rdfs:label "has note on distribution statement"@en,
        "a pour note relative à la mention de diffusion ou de distribution"@fr,
        "har anmärkning om distributionsuppgift"@sv ;
    rdakit:instructionNumber "2.17.8" ;
    rdakit:toolkitDefinition "A note providing details on place of distribution, distributor, or date of distribution, or information on changes in a place of distribution, distributor, or distributor's name."@en,
        "Una nota que proporciona detalles del lugar de distribución, distribuidor o fecha de distribución, o información sobre cambios en el lugar de distribución, distribuidor o nombre del distribuidor."@es,
        "Note fournissant des précisions sur le lieu de diffusion ou de distribution, le diffuseur ou le distributeur ou sur la date de diffusion ou de distribution ou bien de l’information sur les changements de lieu de diffusion ou de distribution, ou de diffuseur ou distributeur ou de nom de diffuseur ou distributeur."@fr ;
    rdakit:toolkitLabel "note on distribution statement"@en,
        "nota sobre la mención de distribución"@es,
        "note relative à la mention de diffusion ou de distribution"@fr,
        "anmärkning om distributionsuppgift"@sv ;
    reg:hasUnconstrained <http://rdaregistry.info/Elements/u/P60125> ;
    reg:lexicalAlias <http://rdaregistry.info/Elements/m/noteOnDistributionStatement.en> ;
    reg:name "noteOnDistributionStatement"@en ;
    reg:status <http://metadataregistry.org/uri/RegStatus/1001> ;
    rdfs:domain <http://rdaregistry.info/Elements/c/C10007> ;
    rdfs:isDefinedBy <http://rdaregistry.info/Elements/m/> ;
    rdfs:subPropertyOf <http://rdaregistry.info/Elements/m/P30137> ;
    skos:definition "Relates a manifestation to a note providing details on place of distribution, distributor, or date of distribution, or information on changes in a place of distribution, distributor, or distributor's name."@en,
        "Met une manifestation en relation avec une note fournissant des précisions sur le lieu de diffusion ou de distribution, le diffuseur ou le distributeur ou sur la date de diffusion ou de distribution ou bien de l’information sur les changements de lieu de diffusion ou de distribution, ou de diffuseur ou distributeur ou de nom de diffuseur ou distributeur."@fr .

<http://rdaregistry.info/Elements/m/P30053> a rdf:Property ;
    rdfs:label "has note on manufacture statement"@en,
        "a pour note relative à la mention de fabrication"@fr,
        "har anmärkning om tillverkningsuppgift"@sv ;
    rdakit:instructionNumber "2.17.9" ;
    rdakit:toolkitDefinition "A note providing details on place of manufacture, manufacturer, or date of manufacture, or information on changes in a place of manufacture, manufacturer, or manufacturer's name."@en,
        "Una nota que proporciona detalles del lugar de fabricación, fabricantes o fecha de fabricación, o información sobre cambios en el lugar de fabricación, fabricante o fecha fabricación."@es,
        "Note fournissant des précisions sur le lieu de fabrication, le fabricant ou la date de fabrication ou bien de l’information sur les changements de lieu de fabrication, de fabricant ou de nom de fabricant."@fr ;
    rdakit:toolkitLabel "note on manufacture statement"@en,
        "nota sobre la mención de fabricación"@es,
        "note relative à la mention de fabrication"@fr,
        "anmärkning om tillverkningsuppgift"@sv ;
    reg:hasUnconstrained <http://rdaregistry.info/Elements/u/P60126> ;
    reg:lexicalAlias <http://rdaregistry.info/Elements/m/noteOnManufactureStatement.en> ;
    reg:name "noteOnManufactureStatement"@en ;
    reg:status <http://metadataregistry.org/uri/RegStatus/1001> ;
    rdfs:domain <http://rdaregistry.info/Elements/c/C10007> ;
    rdfs:isDefinedBy <http://rdaregistry.info/Elements/m/> ;
    rdfs:subPropertyOf <http://rdaregistry.info/Elements/m/P30137> ;
    skos:definition "Relates a manifestation to a note providing details on place of manufacture, manufacturer, or date of manufacture, or information on changes in a place of manufacture, manufacturer, or manufacturer's name."@en,
        "Met une manifestation en relation avec une note fournissant des précisions sur le lieu de fabrication, le fabricant ou la date de fabrication ou bien de l’information sur les changements de lieu de fabrication, de fabricant ou de nom de fabricant."@fr .

<http://rdaregistry.info/Elements/m/P30054> a rdf:Property ;
    rdfs:label "has note on production statement"@en,
        "a pour note relative à la mention de production"@fr,
        "har anmärkning om produktionsuppgift"@sv ;
    rdakit:instructionNumber "2.17.6" ;
    rdakit:toolkitDefinition "A note providing details on place of production, producer, or date of production, or information on changes in a place of production, producer, or producer's name."@en,
        "Una nota que proporciona detalles del lugar de producción, el productor, o la fecha producción, o información sobre cambios en el lugar de producción, el productor o el nombre del productor."@es,
        "Note fournissant des précisions sur le lieu de production, le producteur ou la date de production ou bien de l’information sur les changements de lieu de production, de producteur ou de nom de producteur."@fr ;
    rdakit:toolkitLabel "note on production statement"@en,
        "nota sobre la mención de producción"@es,
        "note relative à la mention de production"@fr,
        "anmärkning om produktionsuppgift"@sv ;
    reg:hasUnconstrained <http://rdaregistry.info/Elements/u/P60127> ;
    reg:lexicalAlias <http://rdaregistry.info/Elements/m/noteOnProductionStatement.en> ;
    reg:name "noteOnProductionStatement"@en ;
    reg:status <http://metadataregistry.org/uri/RegStatus/1001> ;
    rdfs:domain <http://rdaregistry.info/Elements/c/C10007> ;
    rdfs:isDefinedBy <http://rdaregistry.info/Elements/m/> ;
    rdfs:subPropertyOf <http://rdaregistry.info/Elements/m/P30137> ;
    skos:definition "Relates a manifestation to a note providing details on place of production, producer, or date of production, or information on changes in a place of production, producer, or producer's name."@en,
        "Met une manifestation en relation avec une note fournissant des précisions sur le lieu de production, le producteur ou la date de production ou bien de l’information sur les changements de lieu de production, de producteur ou de nom de producteur."@fr .

<http://rdaregistry.info/Elements/m/P30055> a rdf:Property ;
    rdfs:label "has note on publication statement"@en,
        "a pour note relative à la mention de publication"@fr,
        "har anmärkning om utgivningsuppgift"@sv ;
    rdakit:instructionNumber "2.17.7" ;
    rdakit:toolkitDefinition "A note providing details on place of publication, publisher, or date of publication, or information on changes in a place of publication, publisher, or publisher's name."@en,
        "Una nota que proporciona detalles del lugar de publicación, editor o fecha de publicación, o información sobre cambios en el lugar de publicación, editor o nombre del editor."@es,
        "Note fournissant des précisions sur le lieu de publication, l’éditeur ou la date de publication ou bien de l’information sur les changements de lieu de publication, d’éditeur, ou de nom d’éditeur ou sur les interruptions de publication."@fr ;
    rdakit:toolkitLabel "note on publication statement"@en,
        "nota sobre la mención de publicación"@es,
        "note relative à la mention de publication"@fr,
        "anmärkning om utgivningsuppgift"@sv ;
    reg:hasUnconstrained <http://rdaregistry.info/Elements/u/P60128> ;
    reg:lexicalAlias <http://rdaregistry.info/Elements/m/noteOnPublicationStatement.en> ;
    reg:name "noteOnPublicationStatement"@en ;
    reg:status <http://metadataregistry.org/uri/RegStatus/1001> ;
    rdfs:domain <http://rdaregistry.info/Elements/c/C10007> ;
    rdfs:isDefinedBy <http://rdaregistry.info/Elements/m/> ;
    rdfs:subPropertyOf <http://rdaregistry.info/Elements/m/P30137> ;
    skos:definition "Relates a manifestation to a note providing details on place of publication, publisher, or date of publication, information on changes in a place of publication, publisher, or publisher's name, or on suspension of publication."@en,
        "Met une manifestation en relation avec une note fournissant des précisions sur le lieu de publication, l’éditeur ou la date de publication ou bien de l’information sur les changements de lieu de publication, d’éditeur, ou de nom d’éditeur ou sur les interruptions de publication."@fr .

<http://rdaregistry.info/Elements/m/P30056> a rdf:Property ;
    rdfs:label "has note on frequency"@en,
        "a pour note relative à la périodicité"@fr,
        "har anmärkning om frekvens"@sv ;
    rdakit:instructionNumber "2.17.12" ;
    rdakit:toolkitDefinition "A note providing details on the currency of the contents, on the frequency of release of issues or parts of a serial or the frequency of updates to an integrating resource, or on changes in frequency."@en,
        "Una nota que proporciona detalles sobre la frecuencia de salida de las entregas o partes de una publicación seriada, la frecuencia de actualizaciones de un recurso integrable, la actualidad de los contenidos, o cambios en la frecuencia."@es,
        "Note fournissant des précisions sur la fraîcheur du contenu, la périodicité des livraisons ou des parties d’une publication en série ou bien sur la périodicité des mises à jour d’une ressource intégratrice ou sur les changements de périodicité."@fr ;
    rdakit:toolkitLabel "note on frequency"@en,
        "nota sobre la frecuencia"@es,
        "note relative à la périodicité"@fr,
        "anmärkning om frekvens"@sv ;
    reg:hasUnconstrained <http://rdaregistry.info/Elements/u/P60129> ;
    reg:lexicalAlias <http://rdaregistry.info/Elements/m/noteOnFrequency.en> ;
    reg:name "noteOnFrequency"@en ;
    reg:status <http://metadataregistry.org/uri/RegStatus/1001> ;
    rdfs:domain <http://rdaregistry.info/Elements/c/C10007> ;
    rdfs:isDefinedBy <http://rdaregistry.info/Elements/m/> ;
    rdfs:subPropertyOf <http://rdaregistry.info/Elements/m/P30137> ;
    skos:definition "Relates a manifestation to a note providing details on the currency of the contents, on the frequency of release of issues or parts of a serial or the frequency of updates to an integrating resource, or on changes in frequency."@en,
        "Met une manifestation en relation avec une note fournissant des précisions sur la fraîcheur du contenu, la périodicité des livraisons ou des parties d’une publication en série ou bien sur la périodicité des mises à jour d’une ressource intégratrice ou sur les changements de périodicité."@fr .

<http://rdaregistry.info/Elements/m/P30057> a rdf:Property ;
    rdfs:label "has note on statement of responsibility"@en,
        "a pour note relative à la mention de responsabilité"@fr,
        "har anmärkning om upphovsuppgift"@sv ;
    rdakit:instructionNumber "2.17.3" ;
    rdakit:toolkitDefinition "A note providing information on an agent not named in a statement of responsibility to whom responsibility for the creation of, or contribution to a realization of, the intellectual or artistic content of a work has been attributed, on variant forms of names appearing in the manifestation, on changes in statements of responsibility, or on other details relating to a statement of responsibility."@en,
        "Una nota que proporciona información sobre una persona, familia, o entidad corporativa no mencionada en una mención de responsabilidad a la que se ha atribuido la responsabilidad por el contenido intelectual o artístico del recurso, formas variantes de los nombres que aparecen en el recurso, cambios en menciones de responsabilidad, u otros detalles relacionados con una mención de responsabilidad."@es,
        "Note fournissant de l’information sur une personne, une famille ou une collectivité qui n’est pas nommée dans une mention de responsabilité et à qui la responsabilité du contenu intellectuel ou artistique a été attribuée ou bien sur les variantes de forme de nom apparaissant sur la ressource, sur les changements de mentions de responsabilité ou bien sur d’autres particularités relatives aux mentions de responsabilité."@fr ;
    rdakit:toolkitLabel "note on statement of responsibility"@en,
        "nota sobre la mención de responsabilidad"@es,
        "note relative à la mention de responsabilité"@fr,
        "anmärkning om upphovsuppgift"@sv ;
    reg:hasUnconstrained <http://rdaregistry.info/Elements/u/P60130> ;
    reg:lexicalAlias <http://rdaregistry.info/Elements/m/noteOnStatementOfResponsibility.en> ;
    reg:name "noteOnStatementOfResponsibility"@en ;
    reg:status <http://metadataregistry.org/uri/RegStatus/1001> ;
    rdfs:domain <http://rdaregistry.info/Elements/c/C10007> ;
    rdfs:isDefinedBy <http://rdaregistry.info/Elements/m/> ;
    rdfs:subPropertyOf <http://rdaregistry.info/Elements/m/P30137> ;
    skos:definition "Relates a manifestation to a note providing information on an agent not named in a statement of responsibility to whom responsibility for the creation of, or contribution to a realization of, the intellectual or artistic content of a work has been attributed, on variant forms of names appearing in the manifestation, on changes in statements of responsibility, or on other details relating to a statement of responsibility."@en,
        "Met une manifestation en relation avec une note fournissant de l’information sur une personne, une famille ou une collectivité qui n’est pas nommée dans une mention de responsabilité et à qui la responsabilité du contenu intellectuel ou artistique a été attribuée ou bien sur les variantes de forme de nom apparaissant sur la ressource, sur les changements de mentions de responsabilité ou bien sur d’autres particularités relatives aux mentions de responsabilité."@fr .

<http://rdaregistry.info/Elements/m/P30058> a rdf:Property ;
    rdfs:label "has note on series statement"@en,
        "a pour note relative à la mention de collection"@fr,
        "har anmärkning om serieuppgift"@sv ;
    rdakit:instructionNumber "2.17.11" ;
    rdakit:toolkitDefinition "A note providing information on complex series statements, on incorrect numbering within series, on changes in series statements, or on other information relating to a series statement."@en,
        "Una nota que proporciona información sobre menciones de serie complejas, numeración incorrecta dentro de la serie, o cambios en menciones de serie."@es,
        "Note fournissant de l’information sur des mentions de collection complexes, une numérotation erronée à l’intérieur de la collection, ou des changements dans les mentions de collection."@fr ;
    rdakit:toolkitLabel "note on series statement"@en,
        "nota sobre la mención de serie"@es,
        "note relative à la mention de collection"@fr,
        "anmärkning om serieuppgift"@sv ;
    reg:hasUnconstrained <http://rdaregistry.info/Elements/u/P60131> ;
    reg:lexicalAlias <http://rdaregistry.info/Elements/m/noteOnSeriesStatement.en> ;
    reg:name "noteOnSeriesStatement"@en ;
    reg:status <http://metadataregistry.org/uri/RegStatus/1001> ;
    rdfs:domain <http://rdaregistry.info/Elements/c/C10007> ;
    rdfs:isDefinedBy <http://rdaregistry.info/Elements/m/> ;
    rdfs:subPropertyOf <http://rdaregistry.info/Elements/m/P30137> ;
    skos:definition "Relates a manifestation to a note providing information on complex series statements, on incorrect numbering within series, on changes in series statements, or on other information relating to a series statement."@en,
        "Met une manifestation en relation avec une note fournissant de l’information sur des mentions de collection complexes, une numérotation erronée à l’intérieur de la collection, ou des changements dans les mentions de collection."@fr .

<http://rdaregistry.info/Elements/m/P30059> a rdf:Property ;
    rdfs:label "has note on copyright date"@en,
        "a pour note relative à la date de copyright"@fr,
        "har anmärkning om copyrightår"@sv ;
    rdakit:instructionNumber "2.17.10" ;
    rdakit:toolkitDefinition "A note providing information on copyright dates not recorded as part of a copyright date element."@en,
        "Una nota que proporciona información sobre las fechas de derechos de autor como parte del elemento fecha de derechos de autor."@es,
        "Note fournissant un complément d’information sur les dates de copyright s’appliquant à divers aspects de la ressource."@fr ;
    rdakit:toolkitLabel "note on copyright date"@en,
        "nota sobre la fecha de copyright"@es,
        "note relative à la date de copyright"@fr,
        "anmärkning om copyrightår"@sv ;
    reg:hasUnconstrained <http://rdaregistry.info/Elements/u/P60132> ;
    reg:lexicalAlias <http://rdaregistry.info/Elements/m/noteOnCopyrightDate.en> ;
    reg:name "noteOnCopyrightDate"@en ;
    reg:status <http://metadataregistry.org/uri/RegStatus/1001> ;
    rdfs:domain <http://rdaregistry.info/Elements/c/C10007> ;
    rdfs:isDefinedBy <http://rdaregistry.info/Elements/m/> ;
    rdfs:subPropertyOf <http://rdaregistry.info/Elements/m/P30137> ;
    skos:definition "Relates a manifestation to a note providing information on copyright dates not recorded as part of a copyright date element."@en,
        "Met une manifestation en relation avec une note fournissant un complément d’information sur les dates de copyright s’appliquant à divers aspects de la ressource."@fr .

<http://rdaregistry.info/Elements/m/P30060> a rdf:Property ;
    rdfs:label "has note on dimensions of manifestation"@en,
        "a pour note sur les dimensions de la manifestation"@fr,
        "har anmärkning om manifestationens mått"@sv ;
    rdakit:instructionNumber "3.21.3" ;
    rdakit:toolkitDefinition "A note providing information on the dimensions of a manifestation that is not recorded as part of a dimensions element."@en,
        "Una nota que proporciona información sobre las dimensiones de la manifestación que no están registradas formalmente como parte del elemento dimensiones."@es,
        "Note fournissant de l’information sur les dimensions d’une manifestation qui n’est pas enregistrée dans l’élément Dimensions."@fr ;
    rdakit:toolkitLabel "note on dimensions of manifestation"@en,
        "nota sobre las dimensiones de la manifestación"@es,
        "note sur les dimensions de la manifestation"@fr,
        "anmärkning om manifestationens mått"@sv ;
    reg:hasUnconstrained <http://rdaregistry.info/Elements/u/P60133> ;
    reg:lexicalAlias <http://rdaregistry.info/Elements/m/noteOnDimensionsOfManifestation.en> ;
    reg:name "noteOnDimensionsOfManifestation"@en ;
    reg:status <http://metadataregistry.org/uri/RegStatus/1001> ;
    rdfs:domain <http://rdaregistry.info/Elements/c/C10007> ;
    rdfs:isDefinedBy <http://rdaregistry.info/Elements/m/> ;
    rdfs:subPropertyOf <http://rdaregistry.info/Elements/m/P30214> ;
    skos:definition "Relates a manifestation to a note providing information on the dimensions of a manifestation that is not recorded as part of a dimensions element."@en,
        "Met une manifestation en relation avec une note fournissant de l’information sur les dimensions d’une manifestation qui n’est pas enregistrée dans l’élément Dimensions."@fr .

<http://rdaregistry.info/Elements/m/P30061> a rdf:Property ;
    rdfs:label "has note on extent of manifestation"@en,
        "a pour note sur l’importance matérielle de la manifestation"@fr,
        "har anmärkning om manifestationens omfång"@sv ;
    rdakit:instructionNumber "3.21.2" ;
    rdakit:toolkitDefinition "A note providing information on the extent of a manifestation that is not recorded as part of an extent element."@en,
        "Una nota que proporciona información sobre la extensión de una manifestación que no está registrada como parte del elemento extensión."@es,
        "Note fournissant de l’information sur l’importance matérielle de la manifestation qui n’est pas enregistrée dans l’élément Importance matérielle."@fr ;
    rdakit:toolkitLabel "note on extent of manifestation"@en,
        "nota sobre la extensión de la manifestación"@es,
        "note sur l’importance matérielle de la manifestation"@fr,
        "anmärkning om manifestationens omfång"@sv ;
    reg:hasUnconstrained <http://rdaregistry.info/Elements/u/P60134> ;
    reg:lexicalAlias <http://rdaregistry.info/Elements/m/noteOnExtentOfManifestation.en> ;
    reg:name "noteOnExtentOfManifestation"@en ;
    reg:status <http://metadataregistry.org/uri/RegStatus/1001> ;
    rdfs:domain <http://rdaregistry.info/Elements/c/C10007> ;
    rdfs:isDefinedBy <http://rdaregistry.info/Elements/m/> ;
    rdfs:subPropertyOf <http://rdaregistry.info/Elements/m/P30214> ;
    skos:definition "Relates a manifestation to a note providing information on the extent of a manifestation that is not recorded as part of an extent element."@en,
        "Met une manifestation en relation avec une note fournissant de l’information sur l’importance matérielle de la manifestation qui n’est pas enregistrée dans l’élément Importance matérielle."@fr .

<http://rdaregistry.info/Elements/m/P30062> a rdf:Property ;
    rdfs:label "has note on numbering of serials"@en,
        "a pour note relative à la numérotation des publications en série"@fr,
        "har anmärkning om numrering av seriella resurser"@sv ;
    rdakit:instructionNumber "2.17.5" ;
    rdakit:toolkitDefinition "A note providing information on the numbering of the first and/or last issue or part, on complex or irregular numbering including numbering errors, on the period covered by a volume, issue, part, etc., or on other information relating to numbering of serials."@en,
        "Una nota que proporciona información sobre la numeración de la primera y/o última entrega o parte, numeración compleja o irregular (incluyendo errores de numeración), o el período cubierto por un volumen, entrega o parte, etc."@es,
        "Note fournissant de l’information sur la numérotation de la première et/ou de la dernière livraison ou partie, sur une numérotation complexe ou irrégulière (y compris les erreurs de numérotation) ou sur la période couverte par un volume, une livraison, une partie, etc."@fr ;
    rdakit:toolkitLabel "note on numbering of serials"@en,
        "nota sobre numeración de las publicaciones seriadas"@es,
        "note relative à la numérotation des publications en série"@fr,
        "anmärkning om numrering av seriella resurser"@sv ;
    reg:hasUnconstrained <http://rdaregistry.info/Elements/u/P60135> ;
    reg:lexicalAlias <http://rdaregistry.info/Elements/m/noteOnNumberingOfSerials.en> ;
    reg:name "noteOnNumberingOfSerials"@en ;
    reg:status <http://metadataregistry.org/uri/RegStatus/1001> ;
    rdfs:domain <http://rdaregistry.info/Elements/c/C10007> ;
    rdfs:isDefinedBy <http://rdaregistry.info/Elements/m/> ;
    rdfs:subPropertyOf <http://rdaregistry.info/Elements/m/P30137> ;
    skos:definition "Relates a manifestation to a note providing information on the numbering of the first and/or last issue or part, on complex or irregular numbering including numbering errors, on the period covered by a volume, issue, part, etc., or on other information relating to numbering of serials."@en,
        "Met une manifestation en relation avec une note fournissant de l’information sur la numérotation de la première et/ou de la dernière livraison ou partie, sur une numérotation complexe ou irrégulière (y compris les erreurs de numérotation) ou sur la période couverte par un volume, une livraison, une partie, etc."@fr .

<http://rdaregistry.info/Elements/m/P30063> a rdf:Property ;
    rdfs:label "has note on title"@en,
        "a pour note relative au titre"@fr,
        "har anmärkning om titel"@sv ;
    rdakit:instructionNumber "2.17.2" ;
    rdakit:toolkitDefinition "A note providing information on the source from which a title was taken, on the date the title was viewed, on variations in titles, on inaccuracies, deletions, etc., or on other information relating to a title."@en,
        "Una nota que proporciona información sobre la fecha en que el título fue revisado, variaciones en los títulos, inexactitudes, supresiones, etc., u otra información relacionada con el título."@es,
        "Note fournissant de l’information sur la source d’où est tiré un titre, la date à laquelle le titre a été vu, les variations dans les titres, les inexactitudes, les suppressions, etc. ou toute autre information relative au titre."@fr ;
    rdakit:toolkitLabel "note on title"@en,
        "nota sobre el título"@es,
        "note relative au titre"@fr,
        "anmärkning om titel"@sv ;
    reg:hasUnconstrained <http://rdaregistry.info/Elements/u/P60136> ;
    reg:lexicalAlias <http://rdaregistry.info/Elements/m/noteOnTitle.en> ;
    reg:name "noteOnTitle"@en ;
    reg:status <http://metadataregistry.org/uri/RegStatus/1001> ;
    rdfs:domain <http://rdaregistry.info/Elements/c/C10007> ;
    rdfs:isDefinedBy <http://rdaregistry.info/Elements/m/> ;
    rdfs:subPropertyOf <http://rdaregistry.info/Elements/m/P30137> ;
    skos:definition "Relates a manifestation to a note providing information on the source from which a title was taken, on the date the title was viewed, on variations in titles, on inaccuracies, deletions, etc., or on other information relating to a title."@en,
        "Met une manifestation en relation avec une note fournissant de l’information sur la source d’où est tiré un titre, la date à laquelle le titre a été vu, les variations dans les titres, les inexactitudes, les suppressions, etc. ou toute autre information relative au titre."@fr .

<http://rdaregistry.info/Elements/m/P30064> a rdf:Property ;
    rdfs:label "has note on edition statement"@en,
        "a pour note relative à la mention d’édition"@fr,
        "har anmärkning om upplageuppgift"@sv ;
    rdakit:instructionNumber "2.17.4" ;
    rdakit:toolkitDefinition "A note providing information on the source of an edition statement, on edition statements relating to issues, parts, etc., on changes in edition statements, or on other information relating to an edition statement."@en,
        "Una nota que proporciona información sobre la fuente de una mención de edición, mención de edición relacionada con entregas, partes, etc., cambios en las menciones de edición, u otra información relacionada con una mención de edición."@es,
        "Note fournissant de l’information sur la source d’une mention d’édition, sur les mentions d’édition relatives aux livraisons, parties, etc. sur les changements dans les mentions d’édition ou bien toute autre information relative à une mention d’édition."@fr ;
    rdakit:toolkitLabel "note on edition statement"@en,
        "nota sobre la mención de edición"@es,
        "note relative à la mention d’édition"@fr,
        "anmärkning om upplageuppgift"@sv ;
    reg:hasUnconstrained <http://rdaregistry.info/Elements/u/P60137> ;
    reg:lexicalAlias <http://rdaregistry.info/Elements/m/noteOnEditionStatement.en> ;
    reg:name "noteOnEditionStatement"@en ;
    reg:status <http://metadataregistry.org/uri/RegStatus/1001> ;
    rdfs:domain <http://rdaregistry.info/Elements/c/C10007> ;
    rdfs:isDefinedBy <http://rdaregistry.info/Elements/m/> ;
    rdfs:subPropertyOf <http://rdaregistry.info/Elements/m/P30137> ;
    skos:definition "Relates a manifestation to a note providing information on the source of an edition statement, on edition statements relating to issues, parts, etc., on changes in edition statements, or on other information relating to an edition statement."@en,
        "Met une manifestation en relation avec une note fournissant de l’information sur la source d’une mention d’édition, sur les mentions d’édition relatives aux livraisons, parties, etc. sur les changements dans les mentions d’édition ou bien toute autre information relative à une mention d’édition."@fr .

<http://rdaregistry.info/Elements/m/P30065> a rdf:Property ;
    rdfs:label "has publisher's number for notated music"@en,
        "a pour numéro d’éditeur pour la musique"@fr,
        "har editionsnummer"@sv ;
    rdakit:instructionNumber "2.15.2" ;
    rdakit:toolkitDefinition "A numbering designation assigned to a notated music manifestation by a publisher."@en,
        "Una designación numérica asignada a un recurso por un editor musical. Este número aparece normalmente en la portada, la carátula y/o primera página de la música."@es,
        "Numérotation attribuée à une ressource par un éditeur de musique et qui figure normalement uniquement sur la page de titre, la couverture et/ou la première page de musique."@fr ;
    rdakit:toolkitLabel "publisher's number for notated music"@en,
        "número del editor para música"@es,
        "numéro d’éditeur pour la musique"@fr,
        "editionsnummer"@sv ;
    reg:hasUnconstrained <http://rdaregistry.info/Elements/u/P60139> ;
    reg:lexicalAlias <http://rdaregistry.info/Elements/m/publishersNumberForNotatedMusic.en> ;
    reg:name "publishersNumberForNotatedMusic"@en ;
    reg:status <http://metadataregistry.org/uri/RegStatus/1001> ;
    rdfs:domain <http://rdaregistry.info/Elements/c/C10007> ;
    rdfs:isDefinedBy <http://rdaregistry.info/Elements/m/> ;
    rdfs:subPropertyOf <http://rdaregistry.info/Elements/m/P30004> ;
    skos:definition "Relates a manifestation to a numbering designation assigned to a notated music manifestation by a publisher."@en,
        "Met une manifestation en relation avec une numérotation attribuée à une ressource par un éditeur de musique et qui figure normalement uniquement sur la page de titre, la couverture et/ou la première page de musique."@fr ;
    skos:scopeNote "A publisher's number for notated music sometimes includes initials, abbreviations, or words identifying the publisher."@en .

<http://rdaregistry.info/Elements/m/P30066> a rdf:Property ;
    rdfs:label "has plate number for notated music"@en,
        "a pour cotage pour la musique"@fr,
        "har plåtnummer"@sv ;
    rdakit:instructionNumber "2.15.3" ;
    rdakit:toolkitDefinition "A numbering designation assigned to a notated music manifestation by a publisher."@en,
        "Una designación de la numeración asignada a un recurso por un editor musical."@es,
        "Numérotation attribuée à une ressource par un éditeur de musique."@fr ;
    rdakit:toolkitLabel "plate number for notated music"@en,
        "número de plancha para música"@es,
        "cotage pour la musique"@fr,
        "plåtnummer"@sv ;
    reg:hasUnconstrained <http://rdaregistry.info/Elements/u/P60140> ;
    reg:lexicalAlias <http://rdaregistry.info/Elements/m/plateNumberForNotatedMusic.en> ;
    reg:name "plateNumberForNotatedMusic"@en ;
    reg:status <http://metadataregistry.org/uri/RegStatus/1001> ;
    rdfs:domain <http://rdaregistry.info/Elements/c/C10007> ;
    rdfs:isDefinedBy <http://rdaregistry.info/Elements/m/> ;
    rdfs:subPropertyOf <http://rdaregistry.info/Elements/m/P30004> ;
    skos:definition "Relates a manifestation to a numbering designation assigned to a notated music manifestation by a publisher."@en,
        "Met une manifestation en relation avec une numérotation attribuée à une ressource par un éditeur de musique."@fr ;
    skos:scopeNote "A plate number for notated music sometimes includes initials, abbreviations, or words identifying the publisher. It is sometimes followed by a number corresponding to the number of pages or plates or a number corresponding to an individual page or plate."@en,
        "La numérotation est habituellement imprimée au bas de chaque page et figure aussi parfois sur la page de titre."@fr .

<http://rdaregistry.info/Elements/m/P30067> a rdf:Property ;
    rdfs:label "has broadcaster"@en,
        "a pour diffuseur"@fr ;
    rdakit:instructionNumber "18.5" ;
    rdakit:toolkitDefinition "An agent involved in broadcasting a manifestation to an audience via radio, television, webcast, etc."@en,
        "Una persona, familia o entidad corporativa involucrada en la emisión de una manifestación para una audiencia mediante la radio, televisión, transmisión virtual, etc."@es,
        "Personne, famille ou collectivité prenant part à la diffusion d’une manifestation à un public par la radio, la télévision, la webdiffusion, etc."@fr ;
    rdakit:toolkitLabel "broadcaster"@en,
        "radiodifusor"@es,
        "diffuseur"@fr ;
    reg:hasSubproperty <http://rdaregistry.info/Elements/m/object/P30067> ;
    reg:hasUnconstrained <http://rdaregistry.info/Elements/u/P60407> ;
    reg:lexicalAlias <http://rdaregistry.info/Elements/m/broadcaster.en> ;
    reg:name "broadcaster"@en ;
    reg:status <http://metadataregistry.org/uri/RegStatus/1001> ;
    rdfs:domain <http://rdaregistry.info/Elements/c/C10007> ;
    rdfs:isDefinedBy <http://rdaregistry.info/Elements/m/> ;
    rdfs:subPropertyOf <http://rdaregistry.info/Elements/m/P30083> ;
    skos:definition "Relates a manifestation to an agent involved in broadcasting a manifestation to an audience via radio, television, webcast, etc."@en,
        "Met une manifestation en relation avec une personne, famille ou collectivité prenant part à la diffusion d’une manifestation à un public par la radio, la télévision, la webdiffusion, etc."@fr .

<http://rdaregistry.info/Elements/m/P30068> a rdf:Property ;
    rdfs:label "has film distributor"@en,
        "a pour distributeur de films"@fr ;
    rdakit:instructionNumber "18.5" ;
    rdakit:toolkitDefinition "An agent involved in distributing a moving image manifestation to theatres or other distribution channels."@en,
        "Una persona, familia o entidad corporativa que interviene en la distribución de una manifestación de imagen en movimiento para salas de cine y otros canales de distribución."@es,
        "Personne, famille ou collectivité prenant part à la distribution d’une manifestation d’images animées aux salles de cinéma ou aux autres réseaux de distribution."@fr ;
    rdakit:toolkitLabel "film distributor"@en,
        "distributor cinematográfico"@es,
        "distributeur de films"@fr ;
    reg:hasSubproperty <http://rdaregistry.info/Elements/m/object/P30068> ;
    reg:hasUnconstrained <http://rdaregistry.info/Elements/u/P60408> ;
    reg:lexicalAlias <http://rdaregistry.info/Elements/m/filmDistributor.en> ;
    reg:name "filmDistributor"@en ;
    reg:status <http://metadataregistry.org/uri/RegStatus/1001> ;
    rdfs:domain <http://rdaregistry.info/Elements/c/C10007> ;
    rdfs:isDefinedBy <http://rdaregistry.info/Elements/m/> ;
    rdfs:subPropertyOf <http://rdaregistry.info/Elements/m/P30080> ;
    skos:definition "Relates a manifestation to an agent involved in distributing a moving image manifestation to theatres or other distribution channels."@en,
        "Met une manifestation en relation avec une personne, famille ou collectivité prenant part à la distribution d’une manifestation d’images animées aux salles de cinéma ou aux autres réseaux de distribution."@fr .

<http://rdaregistry.info/Elements/m/P30069> a rdf:Property ;
    rdfs:label "has book designer"@en,
        "a pour graphiste"@fr ;
    rdakit:instructionNumber "18.5" ;
    rdakit:toolkitDefinition "An agent involved in manufacturing a manifestation by being responsible for the entire graphic design of a book, including arrangement of type and illustration, choice of materials, and process used."@en,
        "Una persona, familia o entidad corporativa que interviene en la fabricación de una manifestación como responsable del diseño gráfico de un libro en su totalidad, incluyendo la disposición de tipografía e ilustración, selección de materiales, y proceso empleado."@es,
        "Personne, famille ou collectivité prenant part à la fabrication d’une manifestation en étant responsable de toute la conception graphique d’un livre, y compris la composition typographique, l’arrangement des illustrations, le choix des matériaux et le processus utilisé."@fr ;
    rdakit:toolkitLabel "book designer"@en,
        "diseñador de libros"@es,
        "graphiste"@fr ;
    reg:hasSubproperty <http://rdaregistry.info/Elements/m/object/P30069> ;
    reg:hasUnconstrained <http://rdaregistry.info/Elements/u/P60409> ;
    reg:lexicalAlias <http://rdaregistry.info/Elements/m/bookDesigner.en> ;
    reg:name "bookDesigner"@en ;
    reg:status <http://metadataregistry.org/uri/RegStatus/1001> ;
    rdfs:domain <http://rdaregistry.info/Elements/c/C10007> ;
    rdfs:isDefinedBy <http://rdaregistry.info/Elements/m/> ;
    rdfs:subPropertyOf <http://rdaregistry.info/Elements/m/P30082> ;
    skos:definition "Relates a manifestation to an agent involved in manufacturing a manifestation by being responsible for the entire graphic design of a book, including arrangement of type and illustration, choice of materials, and process used."@en,
        "Met une manifestation en relation avec une personne, famille ou collectivité prenant part à la fabrication d’une manifestation en étant responsable de toute la conception graphique d’un livre, y compris la composition typographique, l’arrangement des illustrations, le choix des matériaux et le processus utilisé."@fr .

<http://rdaregistry.info/Elements/m/P30070> a rdf:Property ;
    rdfs:label "has engraver"@en,
        "a pour graveur"@fr ;
    rdakit:instructionNumber "18.5" ;
    rdakit:toolkitDefinition "An agent involved in manufacturing a manifestation by cutting letters, figures, etc., on a surface such as a wooden or metal plate used for printing."@en,
        "Una persona, familia o entidad corporativa que interviene en la fabricación de una manifestación cortando letras, figuras, etc., en una superficie utilizada para impresión como puede ser la madera o planchas de metal."@es,
        "Personne, famille ou collectivité prenant part à la fabrication d’une manifestation en gravant des lettres, des figures, etc. sur une surface telle qu’une plaque de bois ou de métal utilisée pour l’impression."@fr ;
    rdakit:toolkitLabel "engraver"@en,
        "grabador"@es,
        "graveur"@fr ;
    reg:hasSubproperty <http://rdaregistry.info/Elements/m/object/P30070> ;
    reg:hasUnconstrained <http://rdaregistry.info/Elements/u/P60410> ;
    reg:lexicalAlias <http://rdaregistry.info/Elements/m/engraver.en> ;
    reg:name "engraver"@en ;
    reg:status <http://metadataregistry.org/uri/RegStatus/1001> ;
    rdfs:domain <http://rdaregistry.info/Elements/c/C10007> ;
    rdfs:isDefinedBy <http://rdaregistry.info/Elements/m/> ;
    rdfs:subPropertyOf <http://rdaregistry.info/Elements/m/P30082> ;
    skos:definition "Relates a manifestation to an agent involved in manufacturing a manifestation by cutting letters, figures, etc., on a surface such as a wooden or metal plate used for printing."@en,
        "Met une manifestation en relation avec une personne, famille ou collectivité prenant part à la fabrication d’une manifestation en gravant des lettres, des figures, etc. sur une surface telle qu’une plaque de bois ou de métal utilisée pour l’impression."@fr .

<http://rdaregistry.info/Elements/m/P30071> a rdf:Property ;
    rdfs:label "has braille embosser"@en,
        "a pour producteur braille"@fr ;
    rdakit:instructionNumber "18.5" ;
    rdakit:toolkitDefinition "An agent involved in manufacturing a manifestation by embossing braille cells using a stylus, special embossing printer, or other device."@en,
        "Una persona, familia o entidad corporativa que interviene en la fabricación de una manifestación grabando celdas Braille mediante el uso de un punzón, grabador de relieve especial u otro medio."@es,
        "Personne, famille ou collectivité prenant part à la fabrication d’une manifestation par l’embossage de cellules braille au moyen d’un poinçon, d’une imprimante spéciale ou d’un autre appareil."@fr ;
    rdakit:toolkitLabel "braille embosser"@en,
        "grabador de braille"@es,
        "producteur braille"@fr ;
    reg:hasSubproperty <http://rdaregistry.info/Elements/m/object/P30071> ;
    reg:hasUnconstrained <http://rdaregistry.info/Elements/u/P60411> ;
    reg:lexicalAlias <http://rdaregistry.info/Elements/m/brailleEmbosser.en> ;
    reg:name "brailleEmbosser"@en ;
    reg:status <http://metadataregistry.org/uri/RegStatus/1001> ;
    rdfs:domain <http://rdaregistry.info/Elements/c/C10007> ;
    rdfs:isDefinedBy <http://rdaregistry.info/Elements/m/> ;
    rdfs:subPropertyOf <http://rdaregistry.info/Elements/m/P30082> ;
    skos:definition "Relates a manifestation to an agent involved in manufacturing a manifestation by embossing braille cells using a stylus, special embossing printer, or other device."@en,
        "Met une manifestation en relation avec une personne, famille ou collectivité prenant part à la fabrication d’une manifestation par l’embossage de cellules braille au moyen d’un poinçon, d’une imprimante spéciale ou d’un autre appareil."@fr .

<http://rdaregistry.info/Elements/m/P30072> a rdf:Property ;
    rdfs:label "has printmaker"@en,
        "a pour graveur d’estampes"@fr ;
    rdakit:instructionNumber "18.5" ;
    rdakit:toolkitDefinition "An agent involved in manufacturing a manifestation by making a relief, intaglio, or planographic printing surface."@en,
        "Una persona, familia o entidad corporativa que interviene en la fabricación de una manifestación haciendo un relieve, tallado o superficie de impresión planográfica."@es,
        "Personne, famille ou collectivité prenant part à la fabrication d’une manifestation en préparant un élément d’impression en relief, en creux ou planographique."@fr ;
    rdakit:toolkitLabel "printmaker"@en,
        "grabador de estampas"@es,
        "graveur d’estampes"@fr ;
    reg:hasSubproperty <http://rdaregistry.info/Elements/m/object/P30072> ;
    reg:hasUnconstrained <http://rdaregistry.info/Elements/u/P60412> ;
    reg:lexicalAlias <http://rdaregistry.info/Elements/m/printmaker.en> ;
    reg:name "printmaker"@en ;
    reg:status <http://metadataregistry.org/uri/RegStatus/1001> ;
    rdfs:domain <http://rdaregistry.info/Elements/c/C10007> ;
    rdfs:isDefinedBy <http://rdaregistry.info/Elements/m/> ;
    rdfs:subPropertyOf <http://rdaregistry.info/Elements/m/P30082> ;
    skos:definition "Relates a manifestation to an agent involved in manufacturing a manifestation by making a relief, intaglio, or planographic printing surface."@en,
        "Met une manifestation en relation avec une personne, famille ou collectivité prenant part à la fabrication d’une manifestation en préparant un élément d’impression en relief, en creux ou planographique."@fr .

<http://rdaregistry.info/Elements/m/P30073> a rdf:Property ;
    rdfs:label "has caster"@en,
        "a pour fondeur"@fr ;
    rdakit:instructionNumber "18.5" ;
    rdakit:toolkitDefinition "An agent involved in manufacturing a manifestation by pouring a liquid or molten substance into a mold and leaving it to solidify to take the shape of the mold."@en,
        "Una persona, familia o entidad corporativa que interviene en la fabricación de una manifestación mediante el vaciado de un líquido o sustancia derretida en un molde que se deja solidificar hasta tomar la forma de molde."@es,
        "Personne, famille ou collectivité prenant part à la fabrication d’une manifestation en versant un liquide ou une substance fondue dans un moule et en laissant ce liquide ou cette substance se solidifier pour prendre la forme du moule."@fr ;
    rdakit:toolkitLabel "caster"@en,
        "fundidor"@es,
        "fondeur"@fr ;
    reg:hasSubproperty <http://rdaregistry.info/Elements/m/object/P30073> ;
    reg:hasUnconstrained <http://rdaregistry.info/Elements/u/P60413> ;
    reg:lexicalAlias <http://rdaregistry.info/Elements/m/caster.en> ;
    reg:name "caster"@en ;
    reg:status <http://metadataregistry.org/uri/RegStatus/1001> ;
    rdfs:domain <http://rdaregistry.info/Elements/c/C10007> ;
    rdfs:isDefinedBy <http://rdaregistry.info/Elements/m/> ;
    rdfs:subPropertyOf <http://rdaregistry.info/Elements/m/P30082> ;
    skos:definition "Relates a manifestation to an agent involved in manufacturing a manifestation by pouring a liquid or molten substance into a mold and leaving it to solidify to take the shape of the mold."@en,
        "Met une manifestation en relation avec une personne, famille ou collectivité prenant part à la fabrication d’une manifestation en versant un liquide ou une substance fondue dans un moule et en laissant ce liquide ou cette substance se solidifier pour prendre la forme du moule."@fr .

<http://rdaregistry.info/Elements/m/P30074> a rdf:Property ;
    rdfs:label "has lithographer"@en,
        "a pour lithographe"@fr ;
    rdakit:instructionNumber "18.5" ;
    rdakit:toolkitDefinition "An agent involved in manufacturing a manifestation by preparing a stone or plate for lithographic printing."@en,
        "Una persona, familia o entidad corporativa que interviene en la fabricación de una manifestación preparando una piedra o lámina para impresión litográfica, incluyendo al artista gráfico que crea un diseño directamente en la superficie de la cual se hace la impresión."@es,
        "Personne, famille ou collectivité prenant part à la fabrication d’une manifestation en préparant une pierre ou une plaque pour l’impression lithographique, y compris un artiste graphique créant un dessin directement sur la surface à partir de laquelle l’impression sera effectuée."@fr ;
    rdakit:toolkitLabel "lithographer"@en,
        "litógrafo"@es,
        "lithographe"@fr ;
    reg:hasSubproperty <http://rdaregistry.info/Elements/m/object/P30074> ;
    reg:hasUnconstrained <http://rdaregistry.info/Elements/u/P60414> ;
    reg:lexicalAlias <http://rdaregistry.info/Elements/m/lithographer.en> ;
    reg:name "lithographer"@en ;
    reg:status <http://metadataregistry.org/uri/RegStatus/1001> ;
    rdfs:domain <http://rdaregistry.info/Elements/c/C10007> ;
    rdfs:isDefinedBy <http://rdaregistry.info/Elements/m/> ;
    rdfs:subPropertyOf <http://rdaregistry.info/Elements/m/P30082> ;
    skos:definition "Relates a manifestation to an agent involved in manufacturing a manifestation by preparing a stone or plate for lithographic printing."@en,
        "Met une manifestation en relation avec une personne, famille ou collectivité prenant part à la fabrication d’une manifestation en préparant une pierre ou une plaque pour l’impression lithographique, y compris un artiste graphique créant un dessin directement sur la surface à partir de laquelle l’impression sera effectuée."@fr ;
    skos:scopeNote "A lithographer includes a graphic artist creating a design directly on the surface from which printing will be done."@en .

<http://rdaregistry.info/Elements/m/P30075> a rdf:Property ;
    rdfs:label "has platemaker"@en,
        "a pour graveur de planches"@fr ;
    rdakit:instructionNumber "18.5" ;
    rdakit:toolkitDefinition "An agent involved in manufacturing a manifestation by preparing plates used in the production of printed images or text."@en,
        "Una persona, familia o entidad corporativa que interviene en la fabricación de una manifestación preparando planchas utilizadas en la producción de texto e imágenes impresas."@es,
        "Personne, famille ou collectivité prenant part à la fabrication d’une manifestation en préparant les planches utilisées dans la production d’images et/ou de textes imprimés."@fr ;
    rdakit:toolkitLabel "platemaker"@en,
        "grabador de planchas"@es,
        "graveur de planches"@fr ;
    reg:hasSubproperty <http://rdaregistry.info/Elements/m/object/P30075> ;
    reg:hasUnconstrained <http://rdaregistry.info/Elements/u/P60415> ;
    reg:lexicalAlias <http://rdaregistry.info/Elements/m/platemaker.en> ;
    reg:name "platemaker"@en ;
    reg:status <http://metadataregistry.org/uri/RegStatus/1001> ;
    rdfs:domain <http://rdaregistry.info/Elements/c/C10007> ;
    rdfs:isDefinedBy <http://rdaregistry.info/Elements/m/> ;
    rdfs:subPropertyOf <http://rdaregistry.info/Elements/m/P30082> ;
    skos:definition "Relates a manifestation to an agent involved in manufacturing a manifestation by preparing plates used in the production of printed images or text."@en,
        "Met une manifestation en relation avec une personne, famille ou collectivité prenant part à la fabrication d’une manifestation en préparant les planches utilisées dans la production d’images et/ou de textes imprimés."@fr .

<http://rdaregistry.info/Elements/m/P30076> a rdf:Property ;
    rdfs:label "has etcher"@en,
        "a pour aquafortiste"@fr ;
    rdakit:instructionNumber "18.5" ;
    rdakit:toolkitDefinition "An agent involved in manufacturing a manifestation by subjecting metal, glass, or some other surface used for printing, to acid or another corrosive substance."@en,
        "Una persona, familia o entidad corporativa que interviene en la fabricación de una manifestación sometiendo metal, vidrio o alguna otra superficie utilizada para impresión, al contacto con ácido u otra substancia corrosiva."@es,
        "Personne, famille ou collectivité prenant part à la fabrication d’une manifestation en soumettant à l’acide ou à une autre substance corrosive du métal, du verre ou une autre surface utilisée pour l’impression."@fr ;
    rdakit:toolkitLabel "etcher"@en,
        "aguafuertista"@es,
        "aquafortiste"@fr ;
    reg:hasSubproperty <http://rdaregistry.info/Elements/m/object/P30076> ;
    reg:hasUnconstrained <http://rdaregistry.info/Elements/u/P60416> ;
    reg:lexicalAlias <http://rdaregistry.info/Elements/m/etcher.en> ;
    reg:name "etcher"@en ;
    reg:status <http://metadataregistry.org/uri/RegStatus/1001> ;
    rdfs:domain <http://rdaregistry.info/Elements/c/C10007> ;
    rdfs:isDefinedBy <http://rdaregistry.info/Elements/m/> ;
    rdfs:subPropertyOf <http://rdaregistry.info/Elements/m/P30082> ;
    skos:definition "Relates a manifestation to an agent involved in manufacturing a manifestation by subjecting metal, glass, or some other surface used for printing, to acid or another corrosive substance."@en,
        "Met une manifestation en relation avec une personne, famille ou collectivité prenant part à la fabrication d’une manifestation en soumettant à l’acide ou à une autre substance corrosive du métal, du verre ou une autre surface utilisée pour l’impression."@fr .

<http://rdaregistry.info/Elements/m/P30077> a rdf:Property ;
    rdfs:label "has collotyper"@en,
        "a pour phototypeur"@fr ;
    rdakit:instructionNumber "18.5" ;
    rdakit:toolkitDefinition "An agent involved in manufacturing a manifestation by using a photomechanical process for making prints directly from a hardened film of gelatin or other colloid that has ink-receptive and ink-repellent surfaces."@en,
        "Una persona, familia o entidad corporativa que interviene en la fabricación de una manifestación compuesta de impresiones fotográficas sobre película u otro coloide con superficies receptivas y repelentes a la tinta."@es,
        "Personne, famille ou collectivité prenant part à la fabrication d’une manifestation d’épreuves photographiques faites à partir d’un film de gélatine ou d’un autre colloïde ayant des surfaces acceptant ou repoussant l’encre."@fr ;
    rdakit:toolkitLabel "collotyper"@en,
        "fototipista"@es,
        "phototypeur"@fr ;
    reg:hasSubproperty <http://rdaregistry.info/Elements/m/object/P30077> ;
    reg:hasUnconstrained <http://rdaregistry.info/Elements/u/P60417> ;
    reg:lexicalAlias <http://rdaregistry.info/Elements/m/collotyper.en> ;
    reg:name "collotyper"@en ;
    reg:status <http://metadataregistry.org/uri/RegStatus/1001> ;
    rdfs:domain <http://rdaregistry.info/Elements/c/C10007> ;
    rdfs:isDefinedBy <http://rdaregistry.info/Elements/m/> ;
    rdfs:subPropertyOf <http://rdaregistry.info/Elements/m/P30082> ;
    skos:definition "Relates a manifestation to an agent involved in manufacturing a manifestation by using a photomechanical process for making prints directly from a hardened film of gelatin or other colloid that has ink-receptive and ink-repellent surfaces."@en,
        "Met une manifestation en relation avec une personne, famille ou collectivité prenant part à la fabrication d’une manifestation d’épreuves photographiques faites à partir d’un film de gélatine ou d’un autre colloïde ayant des surfaces acceptant ou repoussant l’encre."@fr .

<http://rdaregistry.info/Elements/m/P30078> a rdf:Property ;
    rdfs:label "has printer"@en,
        "a pour imprimeur"@fr ;
    rdakit:instructionNumber "18.5" ;
    rdakit:toolkitDefinition "An agent involved in manufacturing a manifestation of printed text, notated music, etc., from type or plates, such as a book, newspaper, magazine, broadside, score, etc."@en,
        "Una persona, familia o entidad corporativa que interviene en la fabricación de una manifestación de texto impreso, música notada, etc., tal como un libro, periódico, revista, pliego suelto, partitura, etc., mediante tipos o planchas."@es,
        "Personne, famille ou collectivité prenant part à la fabrication d’une manifestation de texte imprimé, de musique notée, etc. à partir de caractères ou de planches, telle qu’un livre, un journal, une revue, un placard, une partition, etc."@fr ;
    rdakit:toolkitLabel "printer"@en,
        "impresor"@es,
        "imprimeur"@fr ;
    reg:hasSubproperty <http://rdaregistry.info/Elements/m/object/P30078> ;
    reg:hasUnconstrained <http://rdaregistry.info/Elements/u/P60418> ;
    reg:lexicalAlias <http://rdaregistry.info/Elements/m/printer.en> ;
    reg:name "printer"@en ;
    reg:status <http://metadataregistry.org/uri/RegStatus/1001> ;
    rdfs:domain <http://rdaregistry.info/Elements/c/C10007> ;
    rdfs:isDefinedBy <http://rdaregistry.info/Elements/m/> ;
    rdfs:subPropertyOf <http://rdaregistry.info/Elements/m/P30082> ;
    skos:definition "Relates a manifestation to an agent involved in manufacturing a manifestation of printed text, notated music, etc., from type or plates, such as a book, newspaper, magazine, broadside, score, etc."@en,
        "Met une manifestation en relation avec une personne, famille ou collectivité prenant part à la fabrication d’une manifestation de texte imprimé, de musique notée, etc. à partir de caractères ou de planches, telle qu’un livre, un journal, une revue, un placard, une partition, etc."@fr .

<http://rdaregistry.info/Elements/m/P30080> a rdf:Property ;
    rdfs:label "has distributor"@en,
        "a pour diffuseur ou distributeur"@fr,
        "har distributör"@sv ;
    rdakit:instructionNumber "21.4" ;
    rdakit:toolkitDefinition "An agent responsible for distributing a manifestation."@en,
        "Una persona, familia o entidad corporativa responsable de la distribución de un recurso."@es,
        "Personne, famille ou collectivité responsable de la diffusion ou de la distribution d’une ressource."@fr ;
    rdakit:toolkitLabel "distributor"@en,
        "distribuidor"@es,
        "diffuseur ou distributeur"@fr,
        "distributör"@sv ;
    reg:hasSubproperty <http://rdaregistry.info/Elements/m/P30068>,
        <http://rdaregistry.info/Elements/m/object/P30080> ;
    reg:hasUnconstrained <http://rdaregistry.info/Elements/u/P60438> ;
    reg:lexicalAlias <http://rdaregistry.info/Elements/m/distributor.en> ;
    reg:name "distributor"@en ;
    reg:status <http://metadataregistry.org/uri/RegStatus/1001> ;
    rdfs:domain <http://rdaregistry.info/Elements/c/C10007> ;
    rdfs:isDefinedBy <http://rdaregistry.info/Elements/m/> ;
    rdfs:subPropertyOf <http://rdaregistry.info/Elements/m/P30267> ;
    skos:definition "Relates a manifestation to an agent responsible for distributing a manifestation."@en,
        "Met une manifestation en relation avec une personne, famille ou collectivité responsable de la diffusion ou de la distribution d’une ressource."@fr .

<http://rdaregistry.info/Elements/m/P30083> a rdf:Property ;
    rdfs:label "has publisher"@en,
        "a pour éditeur"@fr,
        "har utgivare"@sv ;
    rdakit:instructionNumber "21.3" ;
    rdakit:toolkitDefinition "An agent responsible for publishing, releasing, or issuing a manifestation."@en,
        "Una persona, familia o entidad corporativa responsable de la publicación, lanzamiento o publicación de un recurso."@es,
        "Personne, famille ou collectivité responsable de la publication, de la mise à disposition ou de l’édition d’une ressource."@fr ;
    rdakit:toolkitLabel "publisher"@en,
        "editor"@es,
        "éditeur"@fr,
        "utgivare"@sv ;
    reg:hasSubproperty <http://rdaregistry.info/Elements/m/P30067>,
        <http://rdaregistry.info/Elements/m/object/P30083> ;
    reg:hasUnconstrained <http://rdaregistry.info/Elements/u/P60444> ;
    reg:lexicalAlias <http://rdaregistry.info/Elements/m/publisher.en> ;
    reg:name "publisher"@en ;
    reg:status <http://metadataregistry.org/uri/RegStatus/1001> ;
    rdfs:domain <http://rdaregistry.info/Elements/c/C10007> ;
    rdfs:isDefinedBy <http://rdaregistry.info/Elements/m/> ;
    rdfs:subPropertyOf <http://rdaregistry.info/Elements/m/P30267> ;
    skos:definition "Relates a manifestation to an agent responsible for publishing, releasing, or issuing a manifestation."@en,
        "Met une manifestation en relation avec une personne, famille ou collectivité responsable de la publication, de la mise à disposition ou de l’édition d’une ressource."@fr .

<http://rdaregistry.info/Elements/m/P30084> a rdf:Property ;
    rdfs:label "has applied material"@en,
        "a pour matériau appliqué"@fr,
        "har applicerat material"@sv ;
    rdakit:instructionNumber "3.7" ;
    rdakit:toolkitDefinition "A physical or chemical substance applied to a base material of a manifestation."@en,
        "Una sustancia física o química aplicada al material de base de un recurso."@es,
        "Substance physique ou chimique appliquée sur le matériau de base de la ressource."@fr ;
    rdakit:toolkitLabel "applied material"@en,
        "material aplicado"@es,
        "matériau appliqué"@fr,
        "applicerat material"@sv ;
    reg:hasSubproperty <http://rdaregistry.info/Elements/m/P30122> ;
    reg:hasUnconstrained <http://rdaregistry.info/Elements/u/P60159> ;
    reg:lexicalAlias <http://rdaregistry.info/Elements/m/appliedMaterial.en> ;
    reg:name "appliedMaterial"@en ;
    reg:status <http://metadataregistry.org/uri/RegStatus/1001> ;
    rdfs:domain <http://rdaregistry.info/Elements/c/C10007> ;
    rdfs:isDefinedBy <http://rdaregistry.info/Elements/m/> ;
    skos:definition "Relates a manifestation to a physical or chemical substance applied to a base material of a manifestation."@en,
        "Met une manifestation en relation avec une substance physique ou chimique appliquée sur le matériau de base de la ressource."@fr .

<http://rdaregistry.info/Elements/m/P30093> a rdf:Property ;
    rdfs:label "is reprint of (manifestation)"@en,
        "est la réimpression de (manifestation)"@fr ;
    rdakit:instructionNumber "24.5" ;
    rdakit:toolkitDefinition "A printed manifestation that is used as the basis for a reissue of a manifestation."@en,
        "Una manifestación impresa que es usada como base para una reedición de una manifestación."@es,
        "Manifestation imprimée servant de base à une réédition d’une manifestation."@fr ;
    rdakit:toolkitLabel "reprint of (manifestation)"@en,
        "reimpresión de (manifestación)"@es,
        "réimpression de (manifestation)"@fr ;
    reg:hasSubproperty <http://rdaregistry.info/Elements/m/object/P30093> ;
    reg:hasUnconstrained <http://rdaregistry.info/Elements/u/P60168> ;
    reg:lexicalAlias <http://rdaregistry.info/Elements/m/reprintOfManifestation.en> ;
    reg:name "reprintOfManifestation"@en ;
    reg:status <http://metadataregistry.org/uri/RegStatus/1001> ;
    rdfs:domain <http://rdaregistry.info/Elements/c/C10007> ;
    rdfs:isDefinedBy <http://rdaregistry.info/Elements/m/> ;
    rdfs:subPropertyOf <http://rdaregistry.info/Elements/m/P30043> ;
    skos:definition "Relates a manifestation to a printed manifestation that is used as the basis for a reissue of a manifestation."@en,
        "Met une manifestation en relation avec une manifestation imprimée servant de base à une réédition d’une manifestation."@fr .

<http://rdaregistry.info/Elements/m/P30096> a rdf:Property ;
    rdfs:label "has encoding format"@en,
        "a pour format d’encodage"@fr,
        "har kodningsformat"@sv ;
    rdakit:instructionNumber "3.19.3" ;
    rdakit:toolkitDefinition "A schema, standard, etc., used to encode the digital content of a manifestation."@en,
        "Un esquema, estándar, etc., utilizado para codificar el contenido digital de un recurso."@es,
        "Norme, schéma, etc. utilisé pour encoder le contenu numérique d’une ressource."@fr ;
    rdakit:toolkitLabel "encoding format"@en,
        "formato de codificación"@es,
        "format d’encodage"@fr,
        "kodningsformat"@sv ;
    reg:hasUnconstrained <http://rdaregistry.info/Elements/u/P60314> ;
    reg:lexicalAlias <http://rdaregistry.info/Elements/m/encodingFormat.en> ;
    reg:name "encodingFormat"@en ;
    reg:status <http://metadataregistry.org/uri/RegStatus/1001> ;
    rdfs:domain <http://rdaregistry.info/Elements/c/C10007> ;
    rdfs:isDefinedBy <http://rdaregistry.info/Elements/m/> ;
    rdfs:subPropertyOf <http://rdaregistry.info/Elements/m/P30124> ;
    skos:definition "Relates a manifestation to a schema, standard, etc., used to encode the digital content of a manifestation."@en,
        "Met une manifestation en relation avec une norme, un schéma, etc. utilisé pour encoder le contenu numérique d’une ressource."@fr .

<http://rdaregistry.info/Elements/m/P30097> a rdf:Property ;
    rdfs:label "has alternative numeric and/or alphabetic designation of first issue or part of sequence"@en,
        "a pour autre indication numérique et/ou alphabétique de la première livraison ou de la première partie de la séquence"@fr,
        "har alternativ numerisk och/eller alfabetisk beteckning för första numret/delen i svit"@sv ;
    rdakit:instructionNumber "2.6.6" ;
    rdakit:toolkitDefinition "A second or subsequent system of numbering presented in numeric and/or alphabetic form on the first issue or part of a sequence of numbering for a serial."@en,
        "Un segundo o subsecuente sistema de numeración que se presenta en forma numérica y/o alfabética en la primera entrega o parte de una secuencia de numeración para una publicación seriada."@es,
        "Deuxième système de numérotation ou système subséquent présenté sous forme numérique et/ou alphabétique sur la première livraison ou la première partie d’une séquence de numérotation d’une publication en série."@fr ;
    rdakit:toolkitLabel "alternative numeric and/or alphabetic designation of first issue or part of sequence"@en,
        "designación numérica y/o alfabética alternativa de la primera entrega o parte de la secuencia"@es,
        "autre indication numérique et/ou alphabétique de la première livraison ou de la première partie de la séquence"@fr,
        "alternativ numerisk och/eller alfabetisk beteckning för första numret/delen i svit"@sv ;
    reg:hasUnconstrained <http://rdaregistry.info/Elements/u/P60820> ;
    reg:lexicalAlias <http://rdaregistry.info/Elements/m/alternativeNumericAndOrAlphabeticDesignationOfFirstIssueOrPartOfSequence.en> ;
    reg:name "alternativeNumericAndOrAlphabeticDesignationOfFirstIssueOrPartOfSequence"@en ;
    reg:status <http://metadataregistry.org/uri/RegStatus/1001> ;
    rdfs:domain <http://rdaregistry.info/Elements/c/C10007> ;
    rdfs:isDefinedBy <http://rdaregistry.info/Elements/m/> ;
    rdfs:subPropertyOf <http://rdaregistry.info/Elements/m/P30165> ;
    skos:definition "Relates a manifestation to a second or subsequent system of numbering presented in numeric or alphabetic form on the first issue or part of a sequence of numbering for a serial."@en,
        "Met une manifestation en relation avec un deuxième système de numérotation ou un système subséquent présenté sous forme numérique et/ou alphabétique sur la première livraison ou la première partie d’une séquence de numérotation d’une publication en série."@fr .

<http://rdaregistry.info/Elements/m/P30098> a rdf:Property ;
    rdfs:label "has alternative numeric and/or alphabetic designation of last issue or part of sequence"@en,
        "a pour autre indication numérique et/ou alphabétique de la dernière livraison ou de la dernière partie de la séquence"@fr,
        "har alternativ numerisk och/eller alfabetisk beteckning för sista numret/delen i svit"@sv ;
    rdakit:instructionNumber "2.6.8" ;
    rdakit:toolkitDefinition "A second or subsequent system of numbering presented in numeric and/or alphabetic form on the last issue or part of a sequence of numbering for a serial."@en,
        "Un segundo o subsecuente sistema de numeración que se presenta en forma numérica y/o alfabética en la última entrega o parte de una secuencia de numeración para una publicación seriada."@es,
        "Deuxième système de numérotation ou système subséquent présenté sous forme numérique et/ou alphabétique sur la dernière livraison ou la dernière partie d’une séquence de numérotation d’une publication en série."@fr ;
    rdakit:toolkitLabel "alternative numeric and/or alphabetic designation of last issue or part of sequence"@en,
        "designación numérica y/o alfabética alternativa de la última entrega o parte de la secuencia"@es,
        "autre indication numérique et/ou alphabétique de la dernière livraison ou de la dernière partie de la séquence"@fr,
        "alternativ numerisk och/eller alfabetisk beteckning för sista numret/delen i svit"@sv ;
    reg:hasUnconstrained <http://rdaregistry.info/Elements/u/P60821> ;
    reg:lexicalAlias <http://rdaregistry.info/Elements/m/alternativeNumericAndOrAlphabeticDesignationOfLastIssueOrPartOfSequence.en> ;
    reg:name "alternativeNumericAndOrAlphabeticDesignationOfLastIssueOrPartOfSequence"@en ;
    reg:status <http://metadataregistry.org/uri/RegStatus/1001> ;
    rdfs:domain <http://rdaregistry.info/Elements/c/C10007> ;
    rdfs:isDefinedBy <http://rdaregistry.info/Elements/m/> ;
    rdfs:subPropertyOf <http://rdaregistry.info/Elements/m/P30165> ;
    skos:definition "Relates a manifestation to a second or subsequent system of numbering presented in numeric and/or alphabetic form on the last issue or part of a sequence of numbering for a serial."@en,
        "Met une manifestation en relation avec un deuxième système de numérotation ou un système subséquent présenté sous forme numérique et/ou alphabétique sur la dernière livraison ou la dernière partie d’une séquence de numérotation d’une publication en série."@fr .

<http://rdaregistry.info/Elements/m/P30099> a rdf:Property ;
    rdfs:label "has alternative chronological designation of first issue or part of sequence"@en,
        "a pour autre indication chronologique de la première livraison ou de la première partie de la séquence"@fr ;
    rdakit:instructionNumber "2.6.7" ;
    rdakit:toolkitDefinition "A second or subsequent system of numbering presented in the form of a date on the first issue or part of a sequence of numbering for a serial."@en,
        "Un segundo o subsecuente sistema de numeración que se presenta en forma de fecha (por ej., un año; año y mes; mes, día y año) en la primera entrega o parte de una secuencia de numeración para una publicación seriada."@es,
        "Deuxième système de numérotation ou système subséquent présenté sous la forme d’une date (par exemple, année ; année et mois ; mois, jour et année) sur la première livraison ou la première partie d’une séquence de numérotation d’une publication en série."@fr ;
    rdakit:toolkitLabel "alternative chronological designation of first issue or part of sequence"@en,
        "designación cronológica alternativa de la primera entrega o parte de la secuencia"@es,
        "autre indication chronologique de la première livraison ou de la première partie de la séquence"@fr ;
    reg:hasUnconstrained <http://rdaregistry.info/Elements/u/P60818> ;
    reg:lexicalAlias <http://rdaregistry.info/Elements/m/alternativeChronologicalDesignationOfFirstIssueOrPartOfSequence.en> ;
    reg:name "alternativeChronologicalDesignationOfFirstIssueOrPartOfSequence"@en ;
    reg:status <http://metadataregistry.org/uri/RegStatus/1001> ;
    rdfs:domain <http://rdaregistry.info/Elements/c/C10007> ;
    rdfs:isDefinedBy <http://rdaregistry.info/Elements/m/> ;
    rdfs:subPropertyOf <http://rdaregistry.info/Elements/m/P30165> ;
    skos:definition "Relates a manifestation to a second or subsequent system of numbering presented in the form of a date on the first issue or part of a sequence of numbering for a serial."@en,
        "Met une manifestation en relation avec un deuxième système de numérotation ou un système subséquent présenté sous la forme d’une date (par exemple, année ; année et mois ; mois, jour et année) sur la première livraison ou la première partie d’une séquence de numérotation d’une publication en série."@fr ;
    skos:scopeNote "Designation includes a year; year and month; month, day, and year. An alternative chronological designation may include a date in a different calendar."@en .

<http://rdaregistry.info/Elements/m/P30100> a rdf:Property ;
    rdfs:label "has alternative chronological designation of last issue or part of sequence"@en,
        "a pour autre indication chronologique de la dernière livraison ou de la dernière partie de la séquence"@fr ;
    rdakit:instructionNumber "2.6.9" ;
    rdakit:toolkitDefinition "A second or subsequent system of numbering presented in the form of a date on the last issue or part of a sequence of numbering for a serial."@en,
        "Un segundo o subsecuente sistema de numeración que se presenta en la forma de fecha (por ej., un año; año y mes; mes, día y año) en la última entrega o parte de una secuencia de numeración para una publicación seriada."@es,
        "Deuxième système de numérotation ou système subséquent présenté sous la forme d’une date (par exemple, année ; année et mois ; mois, jour et année) sur la dernière livraison ou la dernière partie d’une séquence de numérotation d’une publication en série."@fr ;
    rdakit:toolkitLabel "alternative chronological designation of last issue or part of sequence"@en,
        "designación cronológica alternativa de la última entrega o parte la secuencia"@es,
        "autre indication chronologique de la dernière livraison ou de la dernière partie de la séquence"@fr ;
    reg:hasUnconstrained <http://rdaregistry.info/Elements/u/P60819> ;
    reg:lexicalAlias <http://rdaregistry.info/Elements/m/alternativeChronologicalDesignationOfLastIssueOrPartOfSequence.en> ;
    reg:name "alternativeChronologicalDesignationOfLastIssueOrPartOfSequence"@en ;
    reg:status <http://metadataregistry.org/uri/RegStatus/1001> ;
    rdfs:domain <http://rdaregistry.info/Elements/c/C10007> ;
    rdfs:isDefinedBy <http://rdaregistry.info/Elements/m/> ;
    rdfs:subPropertyOf <http://rdaregistry.info/Elements/m/P30165> ;
    skos:definition "Relates a manifestation to a second or subsequent system of numbering presented in the form of a date on the last issue or part of a sequence of numbering for a serial."@en,
        "Met une manifestation en relation avec un deuxième système de numérotation ou un système subséquent présenté sous la forme d’une date (par exemple, année ; année et mois ; mois, jour et année) sur la dernière livraison ou la dernière partie d’une séquence de numérotation d’une publication en série."@fr ;
    skos:scopeNote "Designation includes a year; year and month; month, day, and year. An alternative chronological designation may include a date in a different calendar."@en .

<http://rdaregistry.info/Elements/m/P30101> a rdf:Property ;
    rdfs:label "is special issue of"@en,
        "est le numéro spécial de"@fr ;
    rdakit:instructionNumber "24.5" ;
    rdakit:toolkitDefinition "A periodical or newspaper containing a single issue or a supplementary section devoted to a special subject, with or without serial numbering."@en,
        "Una publicación seriada o periódico que contiene un número único o sección suplementaria dedicada a un tema especial, con o sin numeración seriada, tal como un número de aniversario de un periódico o revista."@es,
        "Publication en série ou journal contenant un numéro isolé ou un supplément consacré à un sujet spécifique, avec ou sans numérotation, tels qu’un numéro anniversaire d’un périodique ou d’un journal."@fr ;
    rdakit:toolkitLabel "special issue of"@en,
        "número especial de"@es,
        "numéro spécial de"@fr ;
    reg:hasSubproperty <http://rdaregistry.info/Elements/m/object/P30101> ;
    reg:hasUnconstrained <http://rdaregistry.info/Elements/u/P60317> ;
    reg:lexicalAlias <http://rdaregistry.info/Elements/m/specialIssueOf.en> ;
    reg:name "specialIssueOf"@en ;
    reg:status <http://metadataregistry.org/uri/RegStatus/1001> ;
    rdfs:domain <http://rdaregistry.info/Elements/c/C10007> ;
    rdfs:isDefinedBy <http://rdaregistry.info/Elements/m/> ;
    rdfs:subPropertyOf <http://rdaregistry.info/Elements/m/P30020> ;
    skos:definition "Relates a manifestation to a periodical or newspaper containing a single issue or a supplementary section devoted to a special subject, with or without serial numbering."@en,
        "Met une manifestation en relation avec une publication en série ou un journal contenant un numéro isolé ou un supplément consacré à un sujet spécifique, avec ou sans numérotation, tels qu’un numéro anniversaire d’un périodique ou d’un journal."@fr .

<http://rdaregistry.info/Elements/m/P30102> a rdf:Property ;
    rdfs:label "has digital representation of cartographic content"@en,
        "a pour représentation numérique d’un contenu cartographique"@fr ;
    rdakit:instructionNumber "3.19.8" ;
    rdakit:toolkitDefinition "A set of technical details relating to the encoding of geospatial information in a manifestation."@en,
        "Un conjunto de detalles técnicos relacionados con la codificación de información geoespacial en un recurso cartográfico."@es,
        "Ensemble de détails techniques relatifs à l’encodage de l’information géospatiale dans une ressource cartographique."@fr ;
    rdakit:toolkitLabel "digital representation of cartographic content"@en,
        "representación digital de contenido cartográfico"@es,
        "représentation numérique d’un contenu cartographique"@fr ;
    reg:hasUnconstrained <http://rdaregistry.info/Elements/u/P60323> ;
    reg:lexicalAlias <http://rdaregistry.info/Elements/m/digitalRepresentationOfCartographicContent.en> ;
    reg:name "digitalRepresentationOfCartographicContent"@en ;
    reg:status <http://metadataregistry.org/uri/RegStatus/1001> ;
    rdfs:domain <http://rdaregistry.info/Elements/c/C10007> ;
    rdfs:isDefinedBy <http://rdaregistry.info/Elements/m/> ;
    rdfs:subPropertyOf <http://rdaregistry.info/Elements/m/P30124> ;
    skos:definition "Relates a manifestation to a set of technical details relating to the encoding of geospatial information in a manifestation."@en,
        "Met une manifestation en relation avec un ensemble de détails techniques relatifs à l’encodage de l’information géospatiale dans une ressource cartographique."@fr .

<http://rdaregistry.info/Elements/m/P30104> a rdf:Property ;
    rdfs:label "has video format"@en,
        "a pour format vidéo"@fr,
        "har videoformat"@sv ;
    rdakit:instructionNumber "3.18.2" ;
    rdakit:toolkitDefinition "A standard, etc., used to encode the analog video content of a manifestation."@en,
        "Una norma, etc., utilizada para codificar el contenido de vídeo análogo de un recurso."@es,
        "Norme, etc. utilisée pour encoder le contenu vidéo analogique d’une ressource."@fr ;
    rdakit:toolkitLabel "video format"@en,
        "formato de video"@es,
        "format vidéo"@fr,
        "videoformat"@sv ;
    reg:hasUnconstrained <http://rdaregistry.info/Elements/u/P60326> ;
    reg:lexicalAlias <http://rdaregistry.info/Elements/m/videoFormat.en> ;
    reg:name "videoFormat"@en ;
    reg:status <http://metadataregistry.org/uri/RegStatus/1001> ;
    rdfs:domain <http://rdaregistry.info/Elements/c/C10007> ;
    rdfs:isDefinedBy <http://rdaregistry.info/Elements/m/> ;
    rdfs:subPropertyOf <http://rdaregistry.info/Elements/m/P30126> ;
    skos:definition "Relates a manifestation to a standard, etc., used to encode the analog video content of a manifestation."@en,
        "Met une manifestation en relation avec une norme, etc. utilisée pour encoder le contenu vidéo analogique d’une ressource."@fr .

<http://rdaregistry.info/Elements/m/P30105> a rdf:Property ;
    rdfs:label "has statement of responsibility relating to title proper"@en,
        "a pour mention de responsabilité relative au titre propre"@fr,
        "har parallell upphovsuppgift som hänför sig till huvudtiteln"@sv ;
    rdakit:instructionNumber "2.4.2" ;
    rdakit:toolkitDefinition "A statement associated with a title proper of a manifestation that relates to the identification or function of agents responsible for the creation of, or contribution to the realization of, the intellectual or artistic content of a work."@en,
        "Una mención asociada con el título propiamente dicho de un recurso que se relaciona con la identificación y/o función de todas las personas, familias, o entidades corporativas responsables de la creación de, o que contribuyen a la realización del contenido intelectual o artístico del recurso."@es,
        "Mention associée au titre propre d’une ressource et relative à l’identification et/ou la fonction de toute personne, famille ou collectivité responsable de la création, ou ayant contribué à la réalisation du contenu intellectuel ou artistique d’une ressource."@fr ;
    rdakit:toolkitLabel "statement of responsibility relating to title proper"@en,
        "mención de responsabilidad relacionada con el título propiamente dicho"@es,
        "mention de responsabilité relative au titre propre"@fr,
        "parallell upphovsuppgift som hänför sig till huvudtiteln"@sv ;
    reg:hasUnconstrained <http://rdaregistry.info/Elements/u/P60327> ;
    reg:lexicalAlias <http://rdaregistry.info/Elements/m/statementOfResponsibilityRelatingToTitleProper.en> ;
    reg:name "statementOfResponsibilityRelatingToTitleProper"@en ;
    reg:status <http://metadataregistry.org/uri/RegStatus/1001> ;
    rdfs:domain <http://rdaregistry.info/Elements/c/C10007> ;
    rdfs:isDefinedBy <http://rdaregistry.info/Elements/m/> ;
    rdfs:subPropertyOf <http://rdaregistry.info/Elements/m/P30117> ;
    skos:definition "Relates a manifestation to a statement associated with a title proper of a manifestation that relates to the identification or function of agents responsible for the creation of, or contribution to the realization of, the intellectual or artistic content of a work."@en,
        "Met une manifestation en relation avec une mention associée au titre propre d’une ressource et relative à l’identification et/ou la fonction de toute personne, famille ou collectivité responsable de la création, ou ayant contribué à la réalisation du contenu intellectuel ou artistique d’une ressource."@fr .

<http://rdaregistry.info/Elements/m/P30116> a rdf:Property ;
    rdfs:label "has parallel statement of responsibility relating to title proper"@en,
        "a pour mention de responsabilité parallèle relative au titre propre"@fr,
        "har parallell upphovsuppgift som hänför sig till huvudtiteln"@sv ;
    rdakit:instructionNumber "2.4.3" ;
    rdakit:toolkitDefinition "A statement of responsibility relating to title proper in a language or script that differs from that recorded in a statement of responsibility relating to title proper element."@en,
        "Una mención de responsabilidad relacionada con el título propiamente dicho en una lengua y/o escritura que difiere de la registrada en la mención de responsabilidad relacionada con el elemento título propiamente dicho."@es,
        "Mention de responsabilité relative au titre propre dans une langue et/ou une écriture différentes de celles enregistrées dans l’élément Mention de responsabilité relative au titre propre."@fr ;
    rdakit:toolkitLabel "parallel statement of responsibility relating to title proper"@en,
        "mención paralela de responsabilidad relacionada con el título propiamente dicho"@es,
        "mention de responsabilité parallèle relative au titre propre"@fr,
        "parallell upphovsuppgift som hänför sig till huvudtiteln"@sv ;
    reg:hasUnconstrained <http://rdaregistry.info/Elements/u/P60338> ;
    reg:lexicalAlias <http://rdaregistry.info/Elements/m/parallelStatementOfResponsibilityRelatingToTitleProper.en> ;
    reg:name "parallelStatementOfResponsibilityRelatingToTitleProper"@en ;
    reg:status <http://metadataregistry.org/uri/RegStatus/1001> ;
    rdfs:domain <http://rdaregistry.info/Elements/c/C10007> ;
    rdfs:isDefinedBy <http://rdaregistry.info/Elements/m/> ;
    rdfs:subPropertyOf <http://rdaregistry.info/Elements/m/P30117> ;
    skos:definition "Relates a manifestation to a statement of responsibility relating to title proper in a language or script that differs from that recorded in a statement of responsibility relating to title proper element."@en,
        "Met une manifestation en relation avec une mention de responsabilité relative au titre propre dans une langue et/ou une écriture différentes de celles enregistrées dans l’élément Mention de responsabilité relative au titre propre."@fr .

<http://rdaregistry.info/Elements/m/P30122> a rdf:Property ;
    rdfs:label "has emulsion on microfilm and microfiche"@en,
        "a pour émulsion sur microfilm et microfiche"@fr,
        "har emulsion på mikrofilm och mikrofiche"@sv ;
    rdakit:instructionNumber "3.7.2" ;
    rdakit:toolkitDefinition "A suspension of light-sensitive chemicals used as a coating on a microfilm or microfiche."@en,
        "Una suspensión de químicos suaves utilizados como cobertura en un microfilme o una microficha (por ej., haluro de plata)."@es,
        "Suspension de produits chimiques photosensibles utilisés comme revêtement sur un microfilm ou une microfiche (par exemple, l’halogénure d’argent)."@fr ;
    rdakit:toolkitLabel "emulsion on microfilm and microfiche"@en,
        "emulsión en microfilme y microficha"@es,
        "émulsion sur microfilm et microfiche"@fr,
        "emulsion på mikrofilm och mikrofiche"@sv ;
    reg:hasUnconstrained <http://rdaregistry.info/Elements/u/P60344> ;
    reg:lexicalAlias <http://rdaregistry.info/Elements/m/emulsionOnMicrofilmAndMicrofiche.en> ;
    reg:name "emulsionOnMicrofilmAndMicrofiche"@en ;
    reg:status <http://metadataregistry.org/uri/RegStatus/1001> ;
    rdfs:domain <http://rdaregistry.info/Elements/c/C10007> ;
    rdfs:isDefinedBy <http://rdaregistry.info/Elements/m/> ;
    rdfs:subPropertyOf <http://rdaregistry.info/Elements/m/P30084> ;
    skos:definition "Relates a manifestation to a suspension of light-sensitive chemicals used as a coating on a microfilm or microfiche."@en,
        "Met une manifestation en relation avec une suspension de produits chimiques photosensibles utilisés comme revêtement sur un microfilm ou une microfiche (par exemple, l’halogénure d’argent)."@fr .

<http://rdaregistry.info/Elements/m/P30123> a rdf:Property ;
    rdfs:label "has broadcast standard"@en,
        "a pour norme de diffusion"@fr,
        "har sändningsstandard"@sv ;
    rdakit:instructionNumber "3.18.3" ;
    rdakit:toolkitDefinition "A system used to format a manifestation of a video for television broadcast."@en,
        "Un sistema utilizado para formatear un recurso de vídeo para transmisión por televisión."@es,
        "Système utilisé pour formater une ressource vidéo pour la télédiffusion."@fr ;
    rdakit:toolkitLabel "broadcast standard"@en,
        "norma de transmisión"@es,
        "norme de diffusion"@fr,
        "sändningsstandard"@sv ;
    reg:hasUnconstrained <http://rdaregistry.info/Elements/u/P60349> ;
    reg:lexicalAlias <http://rdaregistry.info/Elements/m/broadcastStandard.en> ;
    reg:name "broadcastStandard"@en ;
    reg:status <http://metadataregistry.org/uri/RegStatus/1001> ;
    rdfs:domain <http://rdaregistry.info/Elements/c/C10007> ;
    rdfs:isDefinedBy <http://rdaregistry.info/Elements/m/> ;
    rdfs:subPropertyOf <http://rdaregistry.info/Elements/m/P30126> ;
    skos:definition "Relates a manifestation to a system used to format a manifestation of a video for television broadcast."@en,
        "Met une manifestation en relation avec un système utilisé pour formater une ressource vidéo pour la télédiffusion."@fr .

<http://rdaregistry.info/Elements/m/P30128> a rdf:Property ;
    rdfs:label "has variant title"@en,
        "a pour variante de titre"@fr,
        "har varianttitel"@sv ;
    rdakit:instructionNumber "2.3.6" ;
    rdakit:toolkitDefinition "A title associated with a manifestation that differs from a title recorded as a title proper, a parallel title proper, other title information, parallel other title information, earlier title proper, later title proper, key title, or abbreviated title."@en,
        "Un título asociado con un recurso que difiere de un título registrado como el título propiamente dicho, un título paralelo propiamente dicho, información complementaria del título, información complementaria paralela del título, título anterior propiamente dicho, título posterior propiamente dicho, título clave, o título abreviado."@es,
        "Titre associé à une ressource et qui diffère du titre enregistré comme titre propre, titre propre parallèle, complément du titre, complément du titre parallèle, titre propre antérieur, titre propre ultérieur, titre-clé ou titre abrégé."@fr ;
    rdakit:toolkitLabel "variant title"@en,
        "variante del título"@es,
        "variante de titre"@fr,
        "varianttitel"@sv ;
    reg:hasUnconstrained <http://rdaregistry.info/Elements/u/P60355> ;
    reg:lexicalAlias <http://rdaregistry.info/Elements/m/variantTitle.en> ;
    reg:name "variantTitle"@en ;
    reg:status <http://metadataregistry.org/uri/RegStatus/1001> ;
    rdfs:domain <http://rdaregistry.info/Elements/c/C10007> ;
    rdfs:isDefinedBy <http://rdaregistry.info/Elements/m/> ;
    rdfs:subPropertyOf <http://rdaregistry.info/Elements/m/P30134> ;
    skos:definition "Relates a manifestation to a title associated with a manifestation that differs from a title recorded as a title proper, a parallel title proper, other title information, parallel other title information, earlier title proper, later title proper, key title, or abbreviated title."@en,
        "Met une manifestation en relation avec un titre associé à une ressource et qui diffère du titre enregistré comme titre propre, titre propre parallèle, complément du titre, complément du titre parallèle, titre propre antérieur, titre propre ultérieur, titre-clé ou titre abrégé."@fr .

<http://rdaregistry.info/Elements/m/P30131> a rdf:Property ;
    rdfs:label "has abbreviated title"@en,
        "a pour titre abrégé"@fr,
        "har förkortad titel"@sv ;
    rdakit:instructionNumber "2.3.10" ;
    rdakit:toolkitDefinition "A title that has been abbreviated for purposes of indexing or identification."@en,
        "Un título que ha sido abreviado para efectos de indización o identificación."@es,
        "Titre qui a été abrégé à des fins d’indexation ou d’identification."@fr ;
    rdakit:toolkitLabel "abbreviated title"@en,
        "título abreviado"@es,
        "titre abrégé"@fr,
        "förkortad titel"@sv ;
    reg:hasUnconstrained <http://rdaregistry.info/Elements/u/P60359> ;
    reg:lexicalAlias <http://rdaregistry.info/Elements/m/abbreviatedTitle.en> ;
    reg:name "abbreviatedTitle"@en ;
    reg:status <http://metadataregistry.org/uri/RegStatus/1001> ;
    rdfs:domain <http://rdaregistry.info/Elements/c/C10007> ;
    rdfs:isDefinedBy <http://rdaregistry.info/Elements/m/> ;
    rdfs:subPropertyOf <http://rdaregistry.info/Elements/m/P30134> ;
    skos:definition "Relates a manifestation to a title that has been abbreviated for purposes of indexing or identification."@en,
        "Met une manifestation en relation avec un titre qui a été abrégé à des fins d’indexation ou d’identification."@fr .

<http://rdaregistry.info/Elements/m/P30136> a rdf:Property ;
    rdfs:label "is electronic reproduction of (manifestation)"@en,
        "est la reproduction électronique de (manifestation)"@fr ;
    rdakit:instructionNumber "24.5" ;
    rdakit:toolkitDefinition "A manifestation in an analog format that is transferred to a digital format."@en,
        "Una manifestación en un formato analógico que es transferida a un formato digital."@es,
        "Manifestation sur un support analogique qui a été transférée dans un format numérique."@fr ;
    rdakit:toolkitLabel "electronic reproduction of (manifestation)"@en,
        "reproducción electrónica de (manifestación)"@es,
        "reproduction électronique de (manifestation)"@fr ;
    reg:hasSubproperty <http://rdaregistry.info/Elements/m/object/P30136> ;
    reg:hasUnconstrained <http://rdaregistry.info/Elements/u/P60469> ;
    reg:lexicalAlias <http://rdaregistry.info/Elements/m/electronicReproductionOfManifestation.en> ;
    reg:name "electronicReproductionOfManifestation"@en ;
    reg:status <http://metadataregistry.org/uri/RegStatus/1001> ;
    rdfs:domain <http://rdaregistry.info/Elements/c/C10007> ;
    rdfs:isDefinedBy <http://rdaregistry.info/Elements/m/> ;
    rdfs:subPropertyOf <http://rdaregistry.info/Elements/m/P30043> ;
    skos:definition "Relates a manifestation to a manifestation in an analog format that is transferred to a digital format."@en,
        "Met une manifestation en relation avec une manifestation sur un support analogique qui a été transférée dans un format numérique."@fr .

<http://rdaregistry.info/Elements/m/P30138> a rdf:Property ;
    rdfs:label "has special playback characteristic"@en,
        "a pour caractéristique de lecture particulière"@fr,
        "har specifika uppspelningskaraktäristika"@sv ;
    rdakit:instructionNumber "3.16.9" ;
    rdakit:toolkitDefinition "An equalization system, noise reduction system, etc., used in making an audio recording."@en,
        "Un sistema de ecualización, sistema de reducción del sonido, etc., utilizado en la producción de una grabación de sonido."@es,
        "Système d’égalisation, de réduction du bruit, etc. utilisé pour fabriquer un enregistrement audio."@fr ;
    rdakit:toolkitLabel "special playback characteristic"@en,
        "características especiales de reproducción"@es,
        "caractéristique de lecture particulière"@fr,
        "specifika uppspelningskaraktäristika"@sv ;
    reg:hasUnconstrained <http://rdaregistry.info/Elements/u/P60481> ;
    reg:lexicalAlias <http://rdaregistry.info/Elements/m/specialPlaybackCharacteristic.en> ;
    reg:name "specialPlaybackCharacteristic"@en ;
    reg:status <http://metadataregistry.org/uri/RegStatus/1001> ;
    rdfs:domain <http://rdaregistry.info/Elements/c/C10007> ;
    rdfs:isDefinedBy <http://rdaregistry.info/Elements/m/> ;
    rdfs:subPropertyOf <http://rdaregistry.info/Elements/m/P30125> ;
    skos:definition "Relates a manifestation to an equalization system, noise reduction system, etc., used in making an audio recording."@en,
        "Met une manifestation en relation avec un système d’égalisation, de réduction du bruit, etc. utilisé pour fabriquer un enregistrement audio."@fr .

<http://rdaregistry.info/Elements/m/P30140> a rdf:Property ;
    rdfs:label "has related item (manifestation)"@en,
        "a pour item en relation"@fr,
        "har relaterat exemplar"@sv ;
    rdakit:toolkitDefinition "Un ítem, representado por un identificador o una descripción, que está relacionada con el recurso que se describe (p.ej., un ítem utilizado como base para una reproducción de una microforma)."@es,
        "Item associé à la ressource décrite (par exemple, item utilisé comme base d’une reproduction microforme)."@fr ;
    rdakit:toolkitLabel "ítem relacionado"@es,
        "item en relation"@fr,
        "relaterat exemplar"@sv ;
    reg:hasSubproperty <http://rdaregistry.info/Elements/m/datatype/P30140>,
        <http://rdaregistry.info/Elements/m/object/P30140> ;
    reg:hasUnconstrained <http://rdaregistry.info/Elements/u/P60313> ;
    reg:lexicalAlias <http://rdaregistry.info/Elements/m/relatedItemManifestation.en> ;
    reg:name "relatedItemManifestation"@en ;
    reg:status <http://metadataregistry.org/uri/RegStatus/1001> ;
    rdfs:domain <http://rdaregistry.info/Elements/c/C10007> ;
    rdfs:isDefinedBy <http://rdaregistry.info/Elements/m/> ;
    rdfs:subPropertyOf <http://rdaregistry.info/Elements/m/P30264> ;
    skos:definition "Relates a manifestation to an item associated with a manifestation being described."@en,
        "Met une manifestation en relation avec un item associé à la ressource décrite (par exemple, item utilisé comme base d’une reproduction microforme)."@fr .

<http://rdaregistry.info/Elements/m/P30142> a rdf:Property ;
    rdfs:label "has other title information"@en,
        "a pour complément du titre"@fr,
        "har övrig titelinformation"@sv ;
    rdakit:instructionNumber "2.3.4" ;
    rdakit:toolkitDefinition "A word, character, or group of words or characters that appears in conjunction with, and is subordinate to, a title proper of a manifestation."@en,
        "Información que aparece en conjunción con el título, y está subordinada al título propiamente dicho de un recurso."@es,
        "Information reliée et subordonnée au titre propre d’une ressource."@fr ;
    rdakit:toolkitLabel "other title information"@en,
        "información complementaria del título"@es,
        "complément du titre"@fr,
        "övrig titelinformation"@sv ;
    reg:hasUnconstrained <http://rdaregistry.info/Elements/u/P60493> ;
    reg:lexicalAlias <http://rdaregistry.info/Elements/m/otherTitleInformation.en> ;
    reg:name "otherTitleInformation"@en ;
    reg:status <http://metadataregistry.org/uri/RegStatus/1001> ;
    rdfs:domain <http://rdaregistry.info/Elements/c/C10007> ;
    rdfs:isDefinedBy <http://rdaregistry.info/Elements/m/> ;
    rdfs:subPropertyOf <http://rdaregistry.info/Elements/m/P30134> ;
    skos:definition "Relates a manifestation to a word, character, or group of words or characters that appears in conjunction with, and is subordinate to, a title proper of a manifestation."@en,
        "Met une manifestation en relation avec une information reliée et subordonnée au titre propre d’une ressource."@fr .

<http://rdaregistry.info/Elements/m/P30147> a rdf:Property ;
    rdfs:label "has numeric and/or alphabetic designation of first issue or part of sequence"@en,
        "a pour indication numérique et/ou alphabétique de la première livraison ou de la première partie de la séquence"@fr,
        "har numerisk och/eller alfabetisk beteckning för första numret/delen i svit"@sv ;
    rdakit:instructionNumber "2.6.2" ;
    rdakit:toolkitDefinition "A designation in numeric and/or alphabetic form presented on the first issue or part of a serial issued in a sequence of numbering."@en,
        "Numeración presentada en forma numérica y/o alfabética en la primera entrega o parte de una secuencia de numeración de una publicación seriada."@es,
        "Numérotation présentée sous une forme numérique et/ou alphabétique sur la première livraison ou partie d’une séquence de numérotation pour une publication en série."@fr ;
    rdakit:toolkitLabel "numeric and/or alphabetic designation of first issue or part of sequence"@en,
        "designación numérica y/o alfabética de la primera entrega o parte de la secuencia"@es,
        "indication numérique et/ou alphabétique de la première livraison ou de la première partie de la séquence"@fr,
        "numerisk och/eller alfabetisk beteckning för första numret/delen i svit"@sv ;
    reg:hasUnconstrained <http://rdaregistry.info/Elements/u/P60499> ;
    reg:lexicalAlias <http://rdaregistry.info/Elements/m/numericAndOrAlphabeticDesignationOfFirstIssueOrPartOfSequence.en> ;
    reg:name "numericAndOrAlphabeticDesignationOfFirstIssueOrPartOfSequence"@en ;
    reg:status <http://metadataregistry.org/uri/RegStatus/1001> ;
    rdfs:domain <http://rdaregistry.info/Elements/c/C10007> ;
    rdfs:isDefinedBy <http://rdaregistry.info/Elements/m/> ;
    rdfs:subPropertyOf <http://rdaregistry.info/Elements/m/P30165> ;
    skos:definition "Relates a manifestation to a designation in numeric and/or alphabetic form presented on the first issue or part of a serial issued in a sequence of numbering."@en,
        "Met une manifestation en relation avec une numérotation présentée sous une forme numérique et/ou alphabétique sur la première livraison ou partie d’une séquence de numérotation pour une publication en série."@fr .

<http://rdaregistry.info/Elements/m/P30148> a rdf:Property ;
    rdfs:label "has numeric and/or alphabetic designation of last issue or part of sequence"@en,
        "a pour indication numérique et/ou alphabétique de la dernière livraison ou de la dernière partie de la séquence"@fr,
        "har numerisk och/eller alfabetisk beteckning för sista numret/delen i svit"@sv ;
    rdakit:instructionNumber "2.6.4" ;
    rdakit:toolkitDefinition "A designation in numeric and/or alphabetic form presented on the last issue or part of a serial issued in a sequence of numbering."@en,
        "Numeración presentada en forma numérica y/o alfabética en la última entrega o parte de una secuencia de numeración de una publicación seriada."@es,
        "Numérotation présentée sous une forme numérique et/ou alphabétique sur la dernière livraison ou partie d’une séquence de numérotation pour une publication en série."@fr ;
    rdakit:toolkitLabel "numeric and/or alphabetic designation of last issue or part of sequence"@en,
        "designación numérica y/o alfabética de la última entrega o parte de la secuencia"@es,
        "indication numérique et/ou alphabétique de la dernière livraison ou de la dernière partie de la séquence"@fr,
        "numerisk och/eller alfabetisk beteckning för sista numret/delen i svit"@sv ;
    reg:hasUnconstrained <http://rdaregistry.info/Elements/u/P60500> ;
    reg:lexicalAlias <http://rdaregistry.info/Elements/m/numericAndOrAlphabeticDesignationOfLastIssueOrPartOfSequence.en> ;
    reg:name "numericAndOrAlphabeticDesignationOfLastIssueOrPartOfSequence"@en ;
    reg:status <http://metadataregistry.org/uri/RegStatus/1001> ;
    rdfs:domain <http://rdaregistry.info/Elements/c/C10007> ;
    rdfs:isDefinedBy <http://rdaregistry.info/Elements/m/> ;
    rdfs:subPropertyOf <http://rdaregistry.info/Elements/m/P30165> ;
    skos:definition "Relates a manifestation to a designation in numeric and/or alphabetic form presented on the last issue or part of a serial issued in a sequence of numbering."@en,
        "Met une manifestation en relation avec une numérotation présentée sous une forme numérique et/ou alphabétique sur la dernière livraison ou partie d’une séquence de numérotation pour une publication en série."@fr .

<http://rdaregistry.info/Elements/m/P30149> a rdf:Property ;
    rdfs:label "has chronological designation of first issue or part of sequence"@en,
        "a pour indication chronologique de la première livraison ou de la première partie de la séquence"@fr ;
    rdakit:instructionNumber "2.6.3" ;
    rdakit:toolkitDefinition "A designation in date form presented on the first issue or part of a serial issued in a sequence of numbering."@en,
        "Numeración presentada en forma de fecha (por ej., un año; año y mes; mes, día, y año) en la primera entrega o parte de una secuencia de numeración de una publicación seriada."@es,
        "Numérotation présentée sous la forme d’une date (par exemple, année ; année et mois ; mois, jour et année) sur la première livraison ou la première partie d’une séquence de numérotation d’une publication en série."@fr ;
    rdakit:toolkitLabel "chronological designation of first issue or part of sequence"@en,
        "designación cronológica de la primera entrega o parte de la secuencia"@es,
        "indication chronologique de la première livraison ou de la première partie de la séquence"@fr ;
    reg:hasUnconstrained <http://rdaregistry.info/Elements/u/P60501> ;
    reg:lexicalAlias <http://rdaregistry.info/Elements/m/chronologicalDesignationOfFirstIssueOrPartOfSequence.en> ;
    reg:name "chronologicalDesignationOfFirstIssueOrPartOfSequence"@en ;
    reg:status <http://metadataregistry.org/uri/RegStatus/1001> ;
    rdfs:domain <http://rdaregistry.info/Elements/c/C10007> ;
    rdfs:isDefinedBy <http://rdaregistry.info/Elements/m/> ;
    rdfs:subPropertyOf <http://rdaregistry.info/Elements/m/P30165> ;
    skos:definition "Relates a manifestation to a designation in date form presented on the first issue or part of a serial issued in a sequence of numbering."@en,
        "Met une manifestation en relation avec une numérotation présentée sous la forme d’une date (par exemple, année ; année et mois ; mois, jour et année) sur la première livraison ou la première partie d’une séquence de numérotation d’une publication en série."@fr ;
    skos:scopeNote "Designation includes a year; year and month; month, day, and year."@en .

<http://rdaregistry.info/Elements/m/P30150> a rdf:Property ;
    rdfs:label "has chronological designation of last issue or part of sequence"@en,
        "a pour indication chronologique de la dernière livraison ou de la dernière partie de la séquence"@fr ;
    rdakit:instructionNumber "2.6.5" ;
    rdakit:toolkitDefinition "A designation in date form presented on the last issue or part of a serial issued in a sequence of numbering."@en,
        "Numeración presentada en forma de fecha (por ej., un año; año y mes; mes, día y año) en la última entrega o parte de una secuencia de numeración de una publicación seriada."@es,
        "Numérotation présentée sous la forme d’une date (par exemple, année ; année et mois ; mois, jour et année) sur la dernière livraison ou la dernière partie d’une séquence de numérotation d’une publication en série."@fr ;
    rdakit:toolkitLabel "chronological designation of last issue or part of sequence"@en,
        "designación cronológica de la última entrega o parte de la secuencia"@es,
        "indication chronologique de la dernière livraison ou de la dernière partie de la séquence"@fr ;
    reg:hasUnconstrained <http://rdaregistry.info/Elements/u/P60502> ;
    reg:lexicalAlias <http://rdaregistry.info/Elements/m/chronologicalDesignationOfLastIssueOrPartOfSequence.en> ;
    reg:name "chronologicalDesignationOfLastIssueOrPartOfSequence"@en ;
    reg:status <http://metadataregistry.org/uri/RegStatus/1001> ;
    rdfs:domain <http://rdaregistry.info/Elements/c/C10007> ;
    rdfs:isDefinedBy <http://rdaregistry.info/Elements/m/> ;
    rdfs:subPropertyOf <http://rdaregistry.info/Elements/m/P30165> ;
    skos:definition "Relates a manifestation to a designation in date form presented on the last issue or part of a serial issued in a sequence of numbering."@en,
        "Met une manifestation en relation avec une numérotation présentée sous la forme d’une date (par exemple, année ; année et mois ; mois, jour et année) sur la dernière livraison ou la dernière partie d’une séquence de numérotation d’une publication en série."@fr ;
    skos:scopeNote "Designation includes a year; year and month; month, day, and year."@en .

<http://rdaregistry.info/Elements/m/P30151> a rdf:Property ;
    rdfs:label "has parallel other title information"@en,
        "a pour complément du titre parallèle"@fr,
        "har parallell övrig titelinformation"@sv ;
    rdakit:instructionNumber "2.3.5" ;
    rdakit:toolkitDefinition "An other title information in a language or script that differs from that recorded in an other title information element."@en,
        "Información complementaria del título en una lengua y/o escritura que difiere de la registrada en el elemento información complementaria del título."@es,
        "Complément du titre dans une langue et/ou une écriture différentes de celles enregistrées dans l’élément Complément du titre."@fr ;
    rdakit:toolkitLabel "parallel other title information"@en,
        "información complementaria paralela del título"@es,
        "complément du titre parallèle"@fr,
        "parallell övrig titelinformation"@sv ;
    reg:hasUnconstrained <http://rdaregistry.info/Elements/u/P60507> ;
    reg:lexicalAlias <http://rdaregistry.info/Elements/m/parallelOtherTitleInformation.en> ;
    reg:name "parallelOtherTitleInformation"@en ;
    reg:status <http://metadataregistry.org/uri/RegStatus/1001> ;
    rdfs:domain <http://rdaregistry.info/Elements/c/C10007> ;
    rdfs:isDefinedBy <http://rdaregistry.info/Elements/m/> ;
    rdfs:subPropertyOf <http://rdaregistry.info/Elements/m/P30134> ;
    skos:definition "Relates a manifestation to an other title information in a language or script that differs from that recorded in an other title information element."@en,
        "Met une manifestation en relation avec un complément du titre dans une langue et/ou une écriture différentes de celles enregistrées dans l’élément Complément du titre."@fr .

<http://rdaregistry.info/Elements/m/P30159> a rdf:Property ;
    rdfs:label "has resolution"@en,
        "a pour résolution"@fr,
        "har upplösning"@sv ;
    rdakit:instructionNumber "3.19.5" ;
    rdakit:toolkitDefinition "A clarity or fineness of detail in a digital image, expressed by the measurement of the image in pixels, etc."@en,
        "La claridad o exactitud del detalle en una imagen digital, expresada por la medida de la imagen en pixeles, etc."@es,
        "La netteté ou la finesse de détail d’une image numérique, exprimée par la mesure de l’image en pixels, etc."@fr ;
    rdakit:toolkitLabel "resolution"@en,
        "resolución"@es,
        "résolution"@fr,
        "upplösning"@sv ;
    reg:hasUnconstrained <http://rdaregistry.info/Elements/u/P60519> ;
    reg:lexicalAlias <http://rdaregistry.info/Elements/m/resolution.en> ;
    reg:name "resolution"@en ;
    reg:status <http://metadataregistry.org/uri/RegStatus/1001> ;
    rdfs:domain <http://rdaregistry.info/Elements/c/C10007> ;
    rdfs:isDefinedBy <http://rdaregistry.info/Elements/m/> ;
    rdfs:subPropertyOf <http://rdaregistry.info/Elements/m/P30124> ;
    skos:definition "Relates a manifestation to a clarity or fineness of detail in a digital image, expressed by the measurement of the image in pixels, etc."@en,
        "Met une manifestation en relation avec la netteté ou la finesse de détail d’une image numérique, exprimée par la mesure de l’image en pixels, etc."@fr .

<http://rdaregistry.info/Elements/m/P30161> a rdf:Property ;
    rdfs:label "has track configuration"@en,
        "a pour configuration de piste"@fr,
        "har ljudspårskonfiguration för film"@sv ;
    rdakit:instructionNumber "3.16.6" ;
    rdakit:toolkitDefinition "A configuration of the audio track on a sound-track film."@en,
        "La configuración de la banda de sonido en una película de banda sonora (por ej., pista central)."@es,
        "La configuration de la piste audio sur la bande sonore d’un film (par exemple, piste centrale)."@fr ;
    rdakit:toolkitLabel "track configuration"@en,
        "configuración de banda sonora"@es,
        "configuration de piste"@fr,
        "ljudspårskonfiguration för film"@sv ;
    reg:hasUnconstrained <http://rdaregistry.info/Elements/u/P60522> ;
    reg:lexicalAlias <http://rdaregistry.info/Elements/m/trackConfiguration.en> ;
    reg:name "trackConfiguration"@en ;
    reg:status <http://metadataregistry.org/uri/RegStatus/1001> ;
    rdfs:domain <http://rdaregistry.info/Elements/c/C10007> ;
    rdfs:isDefinedBy <http://rdaregistry.info/Elements/m/> ;
    rdfs:subPropertyOf <http://rdaregistry.info/Elements/m/P30125> ;
    skos:definition "Relates a manifestation to a configuration of the audio track on a sound-track film."@en,
        "Met une manifestation en relation avec la configuration de la piste audio sur la bande sonore d’un film (par exemple, piste centrale)."@fr .

<http://rdaregistry.info/Elements/m/P30163> a rdf:Property ;
    rdfs:label "has presentation format"@en,
        "a pour procédé de projection"@fr,
        "har filmprojektionssystem"@sv ;
    rdakit:instructionNumber "3.17.2" ;
    rdakit:toolkitDefinition "A format used in the production of a projected image."@en,
        "El formato utilizado en la producción de una imagen proyectada (por ej., Cinerama, IMAX)."@es,
        "Le format utilisé pour la production d’une image projetée (par exemple, Cinérama, IMAX)."@fr ;
    rdakit:toolkitLabel "presentation format"@en,
        "formato de presentación"@es,
        "procédé de projection"@fr,
        "filmprojektionssystem"@sv ;
    reg:hasUnconstrained <http://rdaregistry.info/Elements/u/P60529> ;
    reg:lexicalAlias <http://rdaregistry.info/Elements/m/presentationFormat.en> ;
    reg:name "presentationFormat"@en ;
    reg:status <http://metadataregistry.org/uri/RegStatus/1001> ;
    rdfs:domain <http://rdaregistry.info/Elements/c/C10007> ;
    rdfs:isDefinedBy <http://rdaregistry.info/Elements/m/> ;
    rdfs:subPropertyOf <http://rdaregistry.info/Elements/m/P30127> ;
    skos:definition "Relates a manifestation to a format used in the production of a projected image."@en,
        "Met une manifestation en relation avec le format utilisé pour la production d’une image projetée (par exemple, Cinérama, IMAX)."@fr .

<http://rdaregistry.info/Elements/m/P30164> a rdf:Property ;
    rdfs:label "has groove characteristic"@en,
        "a pour caractéristique de sillon"@fr,
        "har spårkarakteristika"@sv ;
    rdakit:instructionNumber "3.16.5" ;
    rdakit:toolkitDefinition "A groove width of an analog disc or a groove pitch of an analog cylinder."@en,
        "La amplitud del surco de un disco análogo o el tono del surco de un cilindro análogo."@es,
        "La largeur de sillon d’un disque analogique ou le pas du sillon d’un cylindre analogique."@fr ;
    rdakit:toolkitLabel "groove characteristic"@en,
        "características del surco"@es,
        "caractéristique de sillon"@fr,
        "spårkarakteristika"@sv ;
    reg:hasUnconstrained <http://rdaregistry.info/Elements/u/P60532> ;
    reg:lexicalAlias <http://rdaregistry.info/Elements/m/grooveCharacteristic.en> ;
    reg:name "grooveCharacteristic"@en ;
    reg:status <http://metadataregistry.org/uri/RegStatus/1001> ;
    rdfs:domain <http://rdaregistry.info/Elements/c/C10007> ;
    rdfs:isDefinedBy <http://rdaregistry.info/Elements/m/> ;
    rdfs:subPropertyOf <http://rdaregistry.info/Elements/m/P30125> ;
    skos:definition "Relates a manifestation to a groove width of an analog disc or a groove pitch of an analog cylinder."@en,
        "Met une manifestation en relation avec la largeur de sillon d’un disque analogique ou le pas du sillon d’un cylindre analogique."@fr .

<http://rdaregistry.info/Elements/m/P30170> a rdf:Property ;
    rdfs:label "has dimensions of map, etc."@en,
        "a pour dimensions d’une carte, etc."@fr,
        "har mått på kartor etc."@sv ;
    rdakit:instructionNumber "3.5.2" ;
    rdakit:toolkitDefinition "A measurement of a face of a map, etc."@en,
        "Las medidas de la cara de un mapa, etc."@es,
        "Les mesures de la surface d’une carte, etc."@fr ;
    rdakit:toolkitLabel "dimensions of map, etc."@en,
        "dimensiones del mapa, etc."@es,
        "dimensions d’une carte, etc."@fr,
        "mått på kartor etc."@sv ;
    reg:hasUnconstrained <http://rdaregistry.info/Elements/u/P60540> ;
    reg:lexicalAlias <http://rdaregistry.info/Elements/m/dimensionsOfMapEtc.en> ;
    reg:name "dimensionsOfMapEtc"@en ;
    reg:status <http://metadataregistry.org/uri/RegStatus/1001> ;
    rdfs:domain <http://rdaregistry.info/Elements/c/C10007> ;
    rdfs:isDefinedBy <http://rdaregistry.info/Elements/m/> ;
    rdfs:subPropertyOf <http://rdaregistry.info/Elements/m/P30169> ;
    skos:definition "Relates a manifestation to a measurement of a face of a map, etc."@en,
        "Met une manifestation en relation avec les mesures de la surface d’une carte, etc."@fr .

<http://rdaregistry.info/Elements/m/P30171> a rdf:Property ;
    rdfs:label "has dimensions of still image"@en,
        "a pour dimensions de l’image fixe"@fr,
        "har bildytans mått"@sv ;
    rdakit:instructionNumber "3.5.3" ;
    rdakit:toolkitDefinition "A measurement of the pictorial area of a still image."@en,
        "La medidas del área pictórica de una imagen fija."@es,
        "Les mesures de la partie graphique d’une image fixe."@fr ;
    rdakit:toolkitLabel "dimensions of still image"@en,
        "dimensiones de la imagen fija"@es,
        "dimensions de l’image fixe"@fr,
        "bildytans mått"@sv ;
    reg:hasUnconstrained <http://rdaregistry.info/Elements/u/P60541> ;
    reg:lexicalAlias <http://rdaregistry.info/Elements/m/dimensionsOfStillImage.en> ;
    reg:name "dimensionsOfStillImage"@en ;
    reg:status <http://metadataregistry.org/uri/RegStatus/1001> ;
    rdfs:domain <http://rdaregistry.info/Elements/c/C10007> ;
    rdfs:isDefinedBy <http://rdaregistry.info/Elements/m/> ;
    rdfs:subPropertyOf <http://rdaregistry.info/Elements/m/P30169> ;
    skos:definition "Relates a manifestation to a measurement of the pictorial area of a still image."@en,
        "Met une manifestation en relation avec les mesures de la partie graphique d’une image fixe."@fr .

<http://rdaregistry.info/Elements/m/P30172> a rdf:Property ;
    rdfs:label "has type of recording"@en,
        "a pour type d’enregistrement"@fr,
        "har inspelningstyp"@sv ;
    rdakit:instructionNumber "3.16.2" ;
    rdakit:toolkitDefinition "A method used to encode audio content for playback."@en,
        "El método utilizado para codificar el contenido sonoro para reproducción (por ej., análogo, digital)."@es,
        "La méthode utilisée pour encoder un contenu audio pour la lecture (par exemple, analogique, numérique)."@fr ;
    rdakit:toolkitLabel "type of recording"@en,
        "tipo de grabación"@es,
        "type d’enregistrement"@fr,
        "inspelningstyp"@sv ;
    reg:hasUnconstrained <http://rdaregistry.info/Elements/u/P60543> ;
    reg:lexicalAlias <http://rdaregistry.info/Elements/m/typeOfRecording.en> ;
    reg:name "typeOfRecording"@en ;
    reg:status <http://metadataregistry.org/uri/RegStatus/1001> ;
    rdfs:domain <http://rdaregistry.info/Elements/c/C10007> ;
    rdfs:isDefinedBy <http://rdaregistry.info/Elements/m/> ;
    rdfs:subPropertyOf <http://rdaregistry.info/Elements/m/P30125> ;
    skos:definition "Relates a manifestation to a method used to encode audio content for playback."@en,
        "Met une manifestation en relation avec la méthode utilisée pour encoder un contenu audio pour la lecture (par exemple, analogique, numérique)."@fr .

<http://rdaregistry.info/Elements/m/P30177> a rdf:Property ;
    rdfs:label "has extent of cartographic resource (Deprecated)"@en,
        "a pour importance matérielle de la ressource cartographique"@fr ;
    rdakit:toolkitDefinition "El número y tipo de unidades y/o subunidades que constituyen un recurso cartográfico."@es,
        "Le nombre et le type d’unités et/ou de sous-unités formant une ressource cartographique."@fr ;
    rdakit:toolkitLabel "extensión de recurso cartográfico"@es,
        "importance matérielle de la ressource cartographique"@fr ;
    reg:hasUnconstrained <http://rdaregistry.info/Elements/u/P60550> ;
    reg:lexicalAlias <http://rdaregistry.info/Elements/m/extentOfCartographicResource.en> ;
    reg:name "extentOfCartographicResource"@en ;
    reg:status <http://metadataregistry.org/uri/RegStatus/1008> ;
    rdfs:domain <http://rdaregistry.info/Elements/c/C10007> ;
    rdfs:isDefinedBy <http://rdaregistry.info/Elements/m/> ;
    rdfs:subPropertyOf <http://rdaregistry.info/Elements/m/P30182> ;
    skos:definition "Met une manifestation en relation avec le nombre et le type d’unités et/ou de sous-unités formant une ressource cartographique."@fr .

<http://rdaregistry.info/Elements/m/P30178> a rdf:Property ;
    rdfs:label "has extent of notated music (Deprecated)"@en,
        "a pour importance matérielle de la musique notée"@fr ;
    rdakit:toolkitDefinition "El número y tipo de unidades y/o subunidades que constituyen un recurso que consiste en música notada (con o sin acompañamiento de texto y/o ilustraciones)."@es,
        "Le nombre et le type d’unités et/ou de sous-unités formant une ressource constituée de musique notée, avec ou sans texte d’accompagnement et/ou illustrations."@fr ;
    rdakit:toolkitLabel "extensión de la música notada"@es,
        "importance matérielle de la musique notée"@fr ;
    reg:hasUnconstrained <http://rdaregistry.info/Elements/u/P60550> ;
    reg:lexicalAlias <http://rdaregistry.info/Elements/m/extentOfNotatedMusic.en> ;
    reg:name "extentOfNotatedMusic"@en ;
    reg:status <http://metadataregistry.org/uri/RegStatus/1008> ;
    rdfs:domain <http://rdaregistry.info/Elements/c/C10007> ;
    rdfs:isDefinedBy <http://rdaregistry.info/Elements/m/> ;
    rdfs:subPropertyOf <http://rdaregistry.info/Elements/m/P30182> ;
    skos:definition "Met une manifestation en relation avec le nombre et le type d’unités et/ou de sous-unités formant une ressource constituée de musique notée, avec ou sans texte d’accompagnement et/ou illustrations."@fr .

<http://rdaregistry.info/Elements/m/P30179> a rdf:Property ;
    rdfs:label "has extent of still image (Deprecated)"@en,
        "a pour importance matérielle de l’image fixe"@fr ;
    rdakit:toolkitDefinition "El número y tipo de unidades y/o subunidades que constituyen un recurso que consiste en una o más imágenes fijas."@es,
        "Le nombre et le type d’unités et/ou de sous-unités formant une ressource constituée d’une ou de plusieurs images fixes."@fr ;
    rdakit:toolkitLabel "extensión de la imagen fija"@es,
        "importance matérielle de l’image fixe"@fr ;
    reg:hasUnconstrained <http://rdaregistry.info/Elements/u/P60550> ;
    reg:lexicalAlias <http://rdaregistry.info/Elements/m/extentOfStillImage.en> ;
    reg:name "extentOfStillImage"@en ;
    reg:status <http://metadataregistry.org/uri/RegStatus/1008> ;
    rdfs:domain <http://rdaregistry.info/Elements/c/C10007> ;
    rdfs:isDefinedBy <http://rdaregistry.info/Elements/m/> ;
    rdfs:subPropertyOf <http://rdaregistry.info/Elements/m/P30182> ;
    skos:definition "Met une manifestation en relation avec le nombre et le type d’unités et/ou de sous-unités formant une ressource constituée d’une ou de plusieurs images fixes."@fr .

<http://rdaregistry.info/Elements/m/P30180> a rdf:Property ;
    rdfs:label "has extent of three-dimensional form (Deprecated)"@en,
        "a pour importance matérielle de la forme tridimensionnelle"@fr ;
    rdakit:toolkitDefinition "El número y tipo de unidades y/o subunidades que constituyen un recurso que consiste en una o más formas tridimensionales."@es,
        "Le nombre et le type d’unités et/ou de sous-unités formant une ressource constituée d’une ou de plusieurs formes tridimensionnelles."@fr ;
    rdakit:toolkitLabel "extensión de la forma tridimensional"@es,
        "importance matérielle de la forme tridimensionnelle"@fr ;
    reg:hasUnconstrained <http://rdaregistry.info/Elements/u/P60550> ;
    reg:lexicalAlias <http://rdaregistry.info/Elements/m/extentOfThreeDimensionalForm.en> ;
    reg:name "extentOfThreeDimensionalForm"@en ;
    reg:status <http://metadataregistry.org/uri/RegStatus/1008> ;
    rdfs:domain <http://rdaregistry.info/Elements/c/C10007> ;
    rdfs:isDefinedBy <http://rdaregistry.info/Elements/m/> ;
    rdfs:subPropertyOf <http://rdaregistry.info/Elements/m/P30182> ;
    skos:definition "Met une manifestation en relation avec le nombre et le type d’unités et/ou de sous-unités formant une ressource constituée d’une ou de plusieurs formes tridimensionnelles."@fr .

<http://rdaregistry.info/Elements/m/P30181> a rdf:Property ;
    rdfs:label "has extent of text (Deprecated)"@en,
        "a pour importance matérielle du texte"@fr ;
    rdakit:toolkitDefinition "El número y tipo de unidades y/o subunidades que constituyen un recurso que consiste en texto (con o sin ilustraciones)."@es,
        "Le nombre et le type d’unités et/ou de sous-unités formant une ressource constituée de texte, avec ou sans illustrations."@fr ;
    rdakit:toolkitLabel "extensión del texto"@es,
        "importance matérielle du texte"@fr ;
    reg:hasUnconstrained <http://rdaregistry.info/Elements/u/P60550> ;
    reg:lexicalAlias <http://rdaregistry.info/Elements/m/extentOfText.en> ;
    reg:name "extentOfText"@en ;
    reg:status <http://metadataregistry.org/uri/RegStatus/1008> ;
    rdfs:domain <http://rdaregistry.info/Elements/c/C10007> ;
    rdfs:isDefinedBy <http://rdaregistry.info/Elements/m/> ;
    rdfs:subPropertyOf <http://rdaregistry.info/Elements/m/P30182> ;
    skos:definition "Met une manifestation en relation avec le nombre et le type d’unités et/ou de sous-unités formant une ressource constituée de texte, avec ou sans illustrations."@fr .

<http://rdaregistry.info/Elements/m/P30183> a rdf:Property ;
    rdfs:label "has file size"@en,
        "a pour taille du fichier"@fr,
        "har filstorlek"@sv ;
    rdakit:instructionNumber "3.19.4" ;
    rdakit:toolkitDefinition "A number of bytes in a digital file."@en,
        "El número de bytes en un archivo digital."@es,
        "Le nombre d’octets d’un fichier numérique."@fr ;
    rdakit:toolkitLabel "file size"@en,
        "tamaño del archivo"@es,
        "taille du fichier"@fr,
        "filstorlek"@sv ;
    reg:hasUnconstrained <http://rdaregistry.info/Elements/u/P60551> ;
    reg:lexicalAlias <http://rdaregistry.info/Elements/m/fileSize.en> ;
    reg:name "fileSize"@en ;
    reg:status <http://metadataregistry.org/uri/RegStatus/1001> ;
    rdfs:domain <http://rdaregistry.info/Elements/c/C10007> ;
    rdfs:isDefinedBy <http://rdaregistry.info/Elements/m/> ;
    rdfs:subPropertyOf <http://rdaregistry.info/Elements/m/P30124> ;
    skos:definition "Relates a manifestation to a number of bytes in a digital file."@en,
        "Met une manifestation en relation avec le nombre d’octets d’un fichier numérique."@fr .

<http://rdaregistry.info/Elements/m/P30184> a rdf:Property ;
    rdfs:label "has configuration of playback channels"@en,
        "a pour configuration des canaux de reproduction"@fr,
        "har antal ljudkanaler"@sv ;
    rdakit:instructionNumber "3.16.8" ;
    rdakit:toolkitDefinition "A number of sound channels used to make a recording."@en,
        "El número de canales sonoros utilizados para hacer una grabación (por ej., un canal para una grabación monofónica, dos canales para una grabación estereofónica)."@es,
        "Le nombre de canaux sonores utilisés pour réaliser un enregistrement (par exemple, un canal pour un enregistrement monophonique, deux canaux pour un enregistrement stéréophonique)."@fr ;
    rdakit:toolkitLabel "configuration of playback channels"@en,
        "configuración de los canales de reproducción sonora"@es,
        "configuration des canaux de reproduction"@fr,
        "antal ljudkanaler"@sv ;
    reg:hasUnconstrained <http://rdaregistry.info/Elements/u/P60552> ;
    reg:lexicalAlias <http://rdaregistry.info/Elements/m/configurationOfPlaybackChannels.en> ;
    reg:name "configurationOfPlaybackChannels"@en ;
    reg:status <http://metadataregistry.org/uri/RegStatus/1001> ;
    rdfs:domain <http://rdaregistry.info/Elements/c/C10007> ;
    rdfs:isDefinedBy <http://rdaregistry.info/Elements/m/> ;
    rdfs:subPropertyOf <http://rdaregistry.info/Elements/m/P30125> ;
    skos:definition "Relates a manifestation to a number of sound channels used to make a recording."@en,
        "Met une manifestation en relation avec le nombre de canaux sonores utilisés pour réaliser un enregistrement (par exemple, un canal pour un enregistrement monophonique, deux canaux pour un enregistrement stéréophonique)."@fr .

<http://rdaregistry.info/Elements/m/P30185> a rdf:Property ;
    rdfs:label "has tape configuration"@en,
        "a pour configuration de bande magnétique"@fr,
        "har antal spår"@sv ;
    rdakit:instructionNumber "3.16.7" ;
    rdakit:toolkitDefinition "A number of tracks on an audiotape."@en,
        "El número de pistas en una cinta de audio."@es,
        "Le nombre de pistes sur une bande audio."@fr ;
    rdakit:toolkitLabel "tape configuration"@en,
        "configuración de cinta"@es,
        "configuration de bande magnétique"@fr,
        "antal spår"@sv ;
    reg:hasUnconstrained <http://rdaregistry.info/Elements/u/P60553> ;
    reg:lexicalAlias <http://rdaregistry.info/Elements/m/tapeConfiguration.en> ;
    reg:name "tapeConfiguration"@en ;
    reg:status <http://metadataregistry.org/uri/RegStatus/1001> ;
    rdfs:domain <http://rdaregistry.info/Elements/c/C10007> ;
    rdfs:isDefinedBy <http://rdaregistry.info/Elements/m/> ;
    rdfs:subPropertyOf <http://rdaregistry.info/Elements/m/P30125> ;
    skos:definition "Relates a manifestation to a number of tracks on an audiotape."@en,
        "Met une manifestation en relation avec le nombre de pistes sur une bande audio."@fr .

<http://rdaregistry.info/Elements/m/P30188> a rdf:Property ;
    rdfs:label "a pour méthode de production d’une ressource tactile"@fr ;
    rdakit:toolkitDefinition "El proceso utilizado para producir un recurso táctil (por ej., repujado, termoformado)."@es,
        "Le procédé utilisé pour produire une ressource tactile (par exemple, embossage, thermoformage)."@fr ;
    rdakit:toolkitLabel "production method for tactile resource"@en,
        "método de producción de un recurso táctil"@es,
        "méthode de production d’une ressource tactile"@fr ;
    reg:hasUnconstrained <http://rdaregistry.info/Elements/u/P60561> ;
    reg:lexicalAlias <http://rdaregistry.info/Elements/m/productionMethodForTactileResource.en> ;
    reg:name "productionMethodForTactileResource"@en ;
    reg:status <http://metadataregistry.org/uri/RegStatus/1008> ;
    rdfs:domain <http://rdaregistry.info/Elements/c/C10007> ;
    rdfs:isDefinedBy <http://rdaregistry.info/Elements/m/> ;
    rdfs:subPropertyOf <http://rdaregistry.info/Elements/m/P30187> ;
    skos:definition "Met une manifestation en relation avec le procédé utilisé pour produire une ressource tactile (par exemple, embossage, thermoformage)."@fr .

<http://rdaregistry.info/Elements/m/P30189> a rdf:Property ;
    rdfs:label "a pour méthode de production d’un manuscrit"@fr ;
    rdakit:toolkitDefinition "The process used to produce an original manuscript or a copy."@en,
        "El proceso utilizado para producir un manuscrito original o una copia."@es,
        "Le procédé utilisé pour produire un manuscrit original ou une copie."@fr ;
    rdakit:toolkitLabel "production method for manuscript"@en,
        "método de producción para un manuscrito"@es,
        "méthode de production d’un manuscrit"@fr ;
    reg:hasUnconstrained <http://rdaregistry.info/Elements/u/P60562> ;
    reg:lexicalAlias <http://rdaregistry.info/Elements/m/productionMethodForManuscript.en> ;
    reg:name "productionMethodForManuscript"@en ;
    reg:status <http://metadataregistry.org/uri/RegStatus/1008> ;
    rdfs:domain <http://rdaregistry.info/Elements/c/C10007> ;
    rdfs:isDefinedBy <http://rdaregistry.info/Elements/m/> ;
    rdfs:subPropertyOf <http://rdaregistry.info/Elements/m/P30187> ;
    skos:definition "Relates a manifestation to the process used to produce an original manuscript or a copy."@en,
        "Met une manifestation en relation avec le procédé utilisé pour produire un manuscrit original ou une copie."@fr .

<http://rdaregistry.info/Elements/m/P30190> a rdf:Property ;
    rdfs:label "a pour génération d’enregistrement audio"@fr ;
    rdakit:toolkitDefinition "La relación entre un soporte de audio original y el soporte de una reproducción hecha del original (por ej., cinta maestra de duplicación, una impresión de prueba)."@es,
        "La relation entre un support matériel original d’un enregistrement audio et le support matériel d’une reproduction faite à partir de l’original (par exemple, une matrice de duplication de bande, un disque-épreuve)."@fr ;
    rdakit:toolkitLabel "generation of audio recording"@en,
        "generación de la grabación sonora"@es,
        "génération d’enregistrement audio"@fr ;
    reg:hasUnconstrained <http://rdaregistry.info/Elements/u/P60567> ;
    reg:lexicalAlias <http://rdaregistry.info/Elements/m/generationOfAudioRecording.en> ;
    reg:name "generationOfAudioRecording"@en ;
    reg:status <http://metadataregistry.org/uri/RegStatus/1008> ;
    rdfs:domain <http://rdaregistry.info/Elements/c/C10007> ;
    rdfs:isDefinedBy <http://rdaregistry.info/Elements/m/> ;
    rdfs:subPropertyOf <http://rdaregistry.info/Elements/m/P30191> ;
    skos:definition "Met une manifestation en relation avec la relation entre un support matériel original d’un enregistrement audio et le support matériel d’une reproduction faite à partir de l’original (par exemple, une matrice de duplication de bande, un disque-épreuve)."@fr .

<http://rdaregistry.info/Elements/m/P30192> a rdf:Property ;
    rdfs:label "a pour génération de ressource numérique"@fr ;
    rdakit:toolkitDefinition "La relación entre el soporte original de un recurso digital y el soporte de una reproducción del original (por ej., máster derivado)."@es,
        "La relation entre un support matériel original d’une ressource numérique et le support matériel d’une reproduction faite à partir de l’original (par exemple, une matrice de dérivation)."@fr ;
    rdakit:toolkitLabel "generation of digital resource"@en,
        "generación del recurso digital"@es,
        "génération de ressource numérique"@fr ;
    reg:hasUnconstrained <http://rdaregistry.info/Elements/u/P60569> ;
    reg:lexicalAlias <http://rdaregistry.info/Elements/m/generationOfDigitalResource.en> ;
    reg:name "generationOfDigitalResource"@en ;
    reg:status <http://metadataregistry.org/uri/RegStatus/1008> ;
    rdfs:domain <http://rdaregistry.info/Elements/c/C10007> ;
    rdfs:isDefinedBy <http://rdaregistry.info/Elements/m/> ;
    rdfs:subPropertyOf <http://rdaregistry.info/Elements/m/P30191> ;
    skos:definition "Met une manifestation en relation avec la relation entre un support matériel original d’une ressource numérique et le support matériel d’une reproduction faite à partir de l’original (par exemple, une matrice de dérivation)."@fr .

<http://rdaregistry.info/Elements/m/P30193> a rdf:Property ;
    rdfs:label "a pour génération de film cinématographique"@fr ;
    rdakit:toolkitDefinition "La relación entre un soporte original de una película cinematográfica como recurso y el soporte de la reproducción hecha del original (por ej., impreso de referencia)."@es,
        "La relation entre un support matériel original d’une ressource filmique et le support matériel d’une reproduction faite à partir de l’original (par exemple, une copie de référence)."@fr ;
    rdakit:toolkitLabel "generation of motion picture film"@en,
        "generación de la película cinematográfica"@es,
        "génération de film cinématographique"@fr ;
    reg:hasUnconstrained <http://rdaregistry.info/Elements/u/P60570> ;
    reg:lexicalAlias <http://rdaregistry.info/Elements/m/generationOfMotionPictureFilm.en> ;
    reg:name "generationOfMotionPictureFilm"@en ;
    reg:status <http://metadataregistry.org/uri/RegStatus/1008> ;
    rdfs:domain <http://rdaregistry.info/Elements/c/C10007> ;
    rdfs:isDefinedBy <http://rdaregistry.info/Elements/m/> ;
    rdfs:subPropertyOf <http://rdaregistry.info/Elements/m/P30191> ;
    skos:definition "Met une manifestation en relation avec la relation entre un support matériel original d’une ressource filmique et le support matériel d’une reproduction faite à partir de l’original (par exemple, une copie de référence)."@fr .

<http://rdaregistry.info/Elements/m/P30194> a rdf:Property ;
    rdfs:label "a pour génération de bande vidéo"@fr ;
    rdakit:toolkitDefinition "La relación entre un soporte original de un recurso en videocinta y el soporte de una reproducción hecha del original (por ej., copia de exhibición)."@es,
        "La relation entre un support matériel original d’une ressource sur bande vidéo et le support matériel d’une reproduction faite à partir de l’original (par exemple, une copie de présentation)."@fr ;
    rdakit:toolkitLabel "generation of videotape"@en,
        "generación de la videocinta"@es,
        "génération de bande vidéo"@fr ;
    reg:hasUnconstrained <http://rdaregistry.info/Elements/u/P60571> ;
    reg:lexicalAlias <http://rdaregistry.info/Elements/m/generationOfVideotape.en> ;
    reg:name "generationOfVideotape"@en ;
    reg:status <http://metadataregistry.org/uri/RegStatus/1008> ;
    rdfs:domain <http://rdaregistry.info/Elements/c/C10007> ;
    rdfs:isDefinedBy <http://rdaregistry.info/Elements/m/> ;
    rdfs:subPropertyOf <http://rdaregistry.info/Elements/m/P30191> ;
    skos:definition "Met une manifestation en relation avec la relation entre un support matériel original d’une ressource sur bande vidéo et le support matériel d’une reproduction faite à partir de l’original (par exemple, une copie de présentation)."@fr .

<http://rdaregistry.info/Elements/m/P30195> a rdf:Property ;
    rdfs:label "a pour génération de microforme"@fr ;
    rdakit:toolkitDefinition "La relación entre el soporte original de una microforma y el soporte de una reproducción hecha del original (por ej., un máster de impresión)."@es,
        "La relation entre un support matériel original d’une ressource sur microforme et le support matériel d’une reproduction faite à partir de l’original (par exemple, matrice)."@fr ;
    rdakit:toolkitLabel "generation of microform"@en,
        "generación de la microforma"@es,
        "génération de microforme"@fr ;
    reg:hasUnconstrained <http://rdaregistry.info/Elements/u/P60572> ;
    reg:lexicalAlias <http://rdaregistry.info/Elements/m/generationOfMicroform.en> ;
    reg:name "generationOfMicroform"@en ;
    reg:status <http://metadataregistry.org/uri/RegStatus/1008> ;
    rdfs:domain <http://rdaregistry.info/Elements/c/C10007> ;
    rdfs:isDefinedBy <http://rdaregistry.info/Elements/m/> ;
    rdfs:subPropertyOf <http://rdaregistry.info/Elements/m/P30191> ;
    skos:definition "Met une manifestation en relation avec la relation entre un support matériel original d’une ressource sur microforme et le support matériel d’une reproduction faite à partir de l’original (par exemple, matrice)."@fr .

<http://rdaregistry.info/Elements/m/P30200> a rdf:Property ;
    rdfs:label "has projection speed"@en,
        "a pour vitesse de projection"@fr,
        "har projektionshastighet"@sv ;
    rdakit:instructionNumber "3.17.3" ;
    rdakit:toolkitDefinition "A speed at which a projected carrier must be operated to produce the moving image intended."@en,
        "La velocidad a la cual un proyector debe ser operado para producir la imagen en movimiento esperada."@es,
        "La vitesse à laquelle doit être actionné un support matériel projeté afin de produire l’image animée prévue."@fr ;
    rdakit:toolkitLabel "projection speed"@en,
        "velocidad de proyección"@es,
        "vitesse de projection"@fr,
        "projektionshastighet"@sv ;
    reg:hasUnconstrained <http://rdaregistry.info/Elements/u/P60585> ;
    reg:lexicalAlias <http://rdaregistry.info/Elements/m/projectionSpeed.en> ;
    reg:name "projectionSpeed"@en ;
    reg:status <http://metadataregistry.org/uri/RegStatus/1001> ;
    rdfs:domain <http://rdaregistry.info/Elements/c/C10007> ;
    rdfs:isDefinedBy <http://rdaregistry.info/Elements/m/> ;
    rdfs:subPropertyOf <http://rdaregistry.info/Elements/m/P30127> ;
    skos:definition "Relates a manifestation to a speed at which a projected carrier must be operated to produce the moving image intended."@en,
        "Met une manifestation en relation avec la vitesse à laquelle doit être actionné un support matériel projeté afin de produire l’image animée prévue."@fr .

<http://rdaregistry.info/Elements/m/P30201> a rdf:Property ;
    rdfs:label "has playing speed"@en,
        "a pour vitesse de lecture"@fr,
        "har uppspelningshastighet"@sv ;
    rdakit:instructionNumber "3.16.4" ;
    rdakit:toolkitDefinition "A speed at which an audio carrier must be operated to produce the sound intended."@en,
        "La velocidad a la cual un soporte de audio debe ser operado para producir el sonido esperado."@es,
        "La vitesse à laquelle un support matériel audio doit être utilisé pour produire le son prévu."@fr ;
    rdakit:toolkitLabel "playing speed"@en,
        "velocidad de reproducción"@es,
        "vitesse de lecture"@fr,
        "uppspelningshastighet"@sv ;
    reg:hasUnconstrained <http://rdaregistry.info/Elements/u/P60586> ;
    reg:lexicalAlias <http://rdaregistry.info/Elements/m/playingSpeed.en> ;
    reg:name "playingSpeed"@en ;
    reg:status <http://metadataregistry.org/uri/RegStatus/1001> ;
    rdfs:domain <http://rdaregistry.info/Elements/c/C10007> ;
    rdfs:isDefinedBy <http://rdaregistry.info/Elements/m/> ;
    rdfs:subPropertyOf <http://rdaregistry.info/Elements/m/P30125> ;
    skos:definition "Relates a manifestation to a speed at which an audio carrier must be operated to produce the sound intended."@en,
        "Met une manifestation en relation avec la vitesse à laquelle un support matériel audio doit être utilisé pour produire le son prévu."@fr .

<http://rdaregistry.info/Elements/m/P30202> a rdf:Property ;
    rdfs:label "has encoded bitrate"@en,
        "a pour débit binaire codé"@fr,
        "har bithastighet"@sv ;
    rdakit:instructionNumber "3.19.7" ;
    rdakit:toolkitDefinition "A speed at which streaming audio, video, etc., is designed to play."@en,
        "La velocidad a la que el streaming de audio, video, etc., está diseñado para funcionar."@es,
        "La vitesse à laquelle un flux audio, vidéo, etc. est destiné à être diffusé."@fr ;
    rdakit:toolkitLabel "encoded bitrate"@en,
        "velocidad de transmisión codificada"@es,
        "débit binaire codé"@fr,
        "bithastighet"@sv ;
    reg:hasUnconstrained <http://rdaregistry.info/Elements/u/P60587> ;
    reg:lexicalAlias <http://rdaregistry.info/Elements/m/encodedBitrate.en> ;
    reg:name "encodedBitrate"@en ;
    reg:status <http://metadataregistry.org/uri/RegStatus/1001> ;
    rdfs:domain <http://rdaregistry.info/Elements/c/C10007> ;
    rdfs:isDefinedBy <http://rdaregistry.info/Elements/m/> ;
    rdfs:subPropertyOf <http://rdaregistry.info/Elements/m/P30124> ;
    skos:definition "Relates a manifestation to a speed at which streaming audio, video, etc., is designed to play."@en,
        "Met une manifestation en relation avec la vitesse à laquelle un flux audio, vidéo, etc. est destiné à être diffusé."@fr .

<http://rdaregistry.info/Elements/m/P30203> a rdf:Property ;
    rdfs:label "has parallel title proper"@en,
        "a pour titre propre parallèle"@fr,
        "har parallell huvudtitel"@sv ;
    rdakit:instructionNumber "2.3.3" ;
    rdakit:toolkitDefinition "A title proper in another language or script."@en,
        "El título propiamente dicho en otra lengua y/o escritura."@es,
        "Le titre propre dans une autre langue et/ou écriture."@fr ;
    rdakit:toolkitLabel "parallel title proper"@en,
        "título paralelo propiamente dicho"@es,
        "titre propre parallèle"@fr,
        "parallell huvudtitel"@sv ;
    reg:hasUnconstrained <http://rdaregistry.info/Elements/u/P60589> ;
    reg:lexicalAlias <http://rdaregistry.info/Elements/m/parallelTitleProper.en> ;
    reg:name "parallelTitleProper"@en ;
    reg:status <http://metadataregistry.org/uri/RegStatus/1001> ;
    rdfs:domain <http://rdaregistry.info/Elements/c/C10007> ;
    rdfs:isDefinedBy <http://rdaregistry.info/Elements/m/> ;
    rdfs:subPropertyOf <http://rdaregistry.info/Elements/m/P30134> ;
    skos:definition "Relates a manifestation to a title proper in another language or script."@en,
        "Met une manifestation en relation avec le titre propre dans une autre langue et/ou écriture."@fr ;
    skos:scopeNote "An alternative title in another language or script is treated as part of a parallel title proper."@en .

<http://rdaregistry.info/Elements/m/P30206> a rdf:Property ;
    rdfs:label "has recording medium"@en,
        "a pour support d’enregistrement"@fr,
        "har inspelningssätt"@sv ;
    rdakit:instructionNumber "3.16.3" ;
    rdakit:toolkitDefinition "A type of medium used to record sound on an audio carrier."@en,
        "El tipo de medio utilizado para grabar el sonido en un soporte de audio (por ej., magnético, óptico)."@es,
        "Le type de support utilisé pour enregistrer du son sur un support matériel audio (par exemple, magnétique, optique)."@fr ;
    rdakit:toolkitLabel "recording medium"@en,
        "medio de grabación"@es,
        "support d’enregistrement"@fr,
        "inspelningssätt"@sv ;
    reg:hasUnconstrained <http://rdaregistry.info/Elements/u/P60594> ;
    reg:lexicalAlias <http://rdaregistry.info/Elements/m/recordingMedium.en> ;
    reg:name "recordingMedium"@en ;
    reg:status <http://metadataregistry.org/uri/RegStatus/1001> ;
    rdfs:domain <http://rdaregistry.info/Elements/c/C10007> ;
    rdfs:isDefinedBy <http://rdaregistry.info/Elements/m/> ;
    rdfs:subPropertyOf <http://rdaregistry.info/Elements/m/P30125> ;
    skos:definition "Relates a manifestation to a type of medium used to record sound on an audio carrier."@en,
        "Met une manifestation en relation avec le type de support utilisé pour enregistrer du son sur un support matériel audio (par exemple, magnétique, optique)."@fr .

<http://rdaregistry.info/Elements/m/P30209> a rdf:Property ;
    rdfs:label "has key title"@en,
        "a pour titre-clé"@fr,
        "har nyckeltitel"@sv ;
    rdakit:instructionNumber "2.3.9" ;
    rdakit:toolkitDefinition "A unique name assigned to a manifestation by an ISSN registration agency."@en,
        "El nombre único asignado a un recurso por una agencia de registro del ISSN."@es,
        "Le nom unique attribué à une ressource par une agence d’enregistrement de l’ISSN."@fr ;
    rdakit:toolkitLabel "key title"@en,
        "título clave"@es,
        "titre-clé"@fr,
        "nyckeltitel"@sv ;
    reg:hasUnconstrained <http://rdaregistry.info/Elements/u/P60597> ;
    reg:lexicalAlias <http://rdaregistry.info/Elements/m/keyTitle.en> ;
    reg:name "keyTitle"@en ;
    reg:status <http://metadataregistry.org/uri/RegStatus/1001> ;
    rdfs:domain <http://rdaregistry.info/Elements/c/C10007> ;
    rdfs:isDefinedBy <http://rdaregistry.info/Elements/m/> ;
    rdfs:subPropertyOf <http://rdaregistry.info/Elements/m/P30134> ;
    skos:definition "Relates a manifestation to a unique name assigned to a manifestation by an ISSN registration agency."@en,
        "Met une manifestation en relation avec le nom unique attribué à une ressource par une agence d’enregistrement de l’ISSN."@fr .

<http://rdaregistry.info/Elements/m/P30215> a rdf:Property ;
    rdfs:label "has papermaker"@en,
        "a pour papetier"@fr ;
    rdakit:instructionNumber "18.5" ;
    rdakit:toolkitDefinition "An agent responsible for the production of paper used to manufacture a manifestation."@en,
        "Una persona, familia o entidad corporativa responsable de la producción del papel usado para fabricar una manifestación."@es,
        "Personne, famille ou collectivité responsable de la production du papier utilisé pour fabriquer une manifestation."@fr ;
    rdakit:toolkitLabel "papermaker"@en,
        "productor de papel"@es,
        "papetier"@fr ;
    reg:hasSubproperty <http://rdaregistry.info/Elements/m/object/P30215> ;
    reg:hasUnconstrained <http://rdaregistry.info/Elements/u/P60746> ;
    reg:lexicalAlias <http://rdaregistry.info/Elements/m/papermaker.en> ;
    reg:name "papermaker"@en ;
    reg:status <http://metadataregistry.org/uri/RegStatus/1001> ;
    rdfs:domain <http://rdaregistry.info/Elements/c/C10007> ;
    rdfs:isDefinedBy <http://rdaregistry.info/Elements/m/> ;
    rdfs:subPropertyOf <http://rdaregistry.info/Elements/m/P30082> ;
    skos:definition "Relates a manifestation to an agent responsible for the production of paper used to manufacture a manifestation."@en,
        "Met une manifestation en relation avec une personne, famille ou collectivité responsable de la production du papier utilisé pour fabriquer une manifestation."@fr .

<http://rdaregistry.info/Elements/m/P30216> a rdf:Property ;
    rdfs:label "has details of applied material"@en,
        "har detaljerad information om applicerat material"@sv ;
    rdakit:instructionNumber "3.7.1.4" ;
    rdakit:toolkitDefinition "Details of a physical or chemical substance applied to a base material of a manifestation."@en,
        "Detalles de una sustancia física o química aplicada al material de base de un recurso."@es ;
    rdakit:toolkitLabel "details of applied material"@en,
        "detalles del material aplicado"@es,
        "detaljerad information om applicerat material"@sv ;
    reg:hasSubproperty <http://rdaregistry.info/Elements/m/P30223> ;
    reg:hasUnconstrained <http://rdaregistry.info/Elements/u/P60767> ;
    reg:lexicalAlias <http://rdaregistry.info/Elements/m/detailsOfAppliedMaterial.en> ;
    reg:name "detailsOfAppliedMaterial"@en ;
    reg:status <http://metadataregistry.org/uri/RegStatus/1001> ;
    rdfs:domain <http://rdaregistry.info/Elements/c/C10007> ;
    rdfs:isDefinedBy <http://rdaregistry.info/Elements/m/> ;
    skos:definition "Relates a manifestation to details of a physical or chemical substance applied to a base material of a manifestation."@en .

<http://rdaregistry.info/Elements/m/P30219> a rdf:Property ;
    rdfs:label "has details of broadcast standard"@en,
        "har detaljerad information om sändningsstandard"@sv ;
    rdakit:instructionNumber "3.18.3.4" ;
    rdakit:toolkitDefinition "Details of a system used to format a manifestation of a video for television broadcast."@en,
        "Detalles de un sistema utilizado para formatear un recurso de vídeo para transmisión por televisión."@es ;
    rdakit:toolkitLabel "details of broadcast standard"@en,
        "detalles de la norma de transmisión"@es,
        "detaljerad information om sändningsstandard"@sv ;
    reg:hasUnconstrained <http://rdaregistry.info/Elements/u/P60770> ;
    reg:lexicalAlias <http://rdaregistry.info/Elements/m/detailsOfBroadcastStandard.en> ;
    reg:name "detailsOfBroadcastStandard"@en ;
    reg:status <http://metadataregistry.org/uri/RegStatus/1001> ;
    rdfs:domain <http://rdaregistry.info/Elements/c/C10007> ;
    rdfs:isDefinedBy <http://rdaregistry.info/Elements/m/> ;
    rdfs:subPropertyOf <http://rdaregistry.info/Elements/m/P30250> ;
    skos:definition "Relates a manifestation to details of a system used to format a manifestation of a video for television broadcast."@en .

<http://rdaregistry.info/Elements/m/P30220> a rdf:Property ;
    rdfs:label "has details of configuration of playback channels"@en,
        "har detaljerad information om antal ljudkanaler"@sv ;
    rdakit:instructionNumber "3.16.8.4" ;
    rdakit:toolkitDefinition "Details of a number of sound channels used to make a recording."@en,
        "Detalles del número de canales sonoros utilizados para hacer una grabación (por ej., un canal para una grabación monofónica, dos canales para una grabación estereofónica)."@es ;
    rdakit:toolkitLabel "details of configuration of playback channels"@en,
        "detalles de la configuración de canales de reproducción"@es,
        "detaljerad information om antal ljudkanaler"@sv ;
    reg:hasUnconstrained <http://rdaregistry.info/Elements/u/P60771> ;
    reg:lexicalAlias <http://rdaregistry.info/Elements/m/detailsOfConfigurationOfPlaybackChannels.en> ;
    reg:name "detailsOfConfigurationOfPlaybackChannels"@en ;
    reg:status <http://metadataregistry.org/uri/RegStatus/1001> ;
    rdfs:domain <http://rdaregistry.info/Elements/c/C10007> ;
    rdfs:isDefinedBy <http://rdaregistry.info/Elements/m/> ;
    rdfs:subPropertyOf <http://rdaregistry.info/Elements/m/P30245> ;
    skos:definition "Relates a manifestation to details of a number of sound channels used to make a recording."@en .

<http://rdaregistry.info/Elements/m/P30222> a rdf:Property ;
    rdfs:label "has details of digital representation of cartographic content"@en,
        "har detaljerad information om geografisk data relaterad till kodningen av en kartografisk resurs"@sv ;
    rdakit:instructionNumber "3.19.8.4" ;
    rdakit:toolkitDefinition "Details of an encoding of geospatial information in a manifestation."@en,
        "Detalles de la codificación de información geoespacial en un recurso cartográfico (p. ej., el nivel topológico, compresión)."@es ;
    rdakit:toolkitLabel "details of digital representation of cartographic content"@en,
        "detalles de la representación digital de contenido cartográfico"@es,
        "detaljerad information om geografisk data relaterad till kodningen av en kartografisk resurs"@sv ;
    reg:hasUnconstrained <http://rdaregistry.info/Elements/u/P60773> ;
    reg:lexicalAlias <http://rdaregistry.info/Elements/m/detailsOfDigitalRepresentationOfCartographicContent.en> ;
    reg:name "detailsOfDigitalRepresentationOfCartographicContent"@en ;
    reg:status <http://metadataregistry.org/uri/RegStatus/1001> ;
    rdfs:domain <http://rdaregistry.info/Elements/c/C10007> ;
    rdfs:isDefinedBy <http://rdaregistry.info/Elements/m/> ;
    rdfs:subPropertyOf <http://rdaregistry.info/Elements/m/P30221> ;
    skos:definition "Relates a manifestation to details of an encoding of geospatial information in a manifestation."@en .

<http://rdaregistry.info/Elements/m/P30223> a rdf:Property ;
    rdfs:label "has details of emulsion on microfilm and microfiche"@en,
        "har detaljerad information om emulsion på microfilm och microfiche"@sv ;
    rdakit:instructionNumber "3.7.2.4" ;
    rdakit:toolkitDefinition "Details of a suspension of light-sensitive chemicals used as a coating on a microfilm or microfiche."@en,
        "Detalles de la suspensión de químicos suaves utilizados como cobertura en un microfilme o una microficha (por ej., haluro de plata)."@es ;
    rdakit:toolkitLabel "details of emulsion on microfilm and microfiche"@en,
        "detalles de la emulsión en el microfilme y la microficha"@es,
        "detaljerad information om emulsion på microfilm och microfiche"@sv ;
    reg:hasUnconstrained <http://rdaregistry.info/Elements/u/P60774> ;
    reg:lexicalAlias <http://rdaregistry.info/Elements/m/detailsOfEmulsionOnMicrofilmAndMicrofiche.en> ;
    reg:name "detailsOfEmulsionOnMicrofilmAndMicrofiche"@en ;
    reg:status <http://metadataregistry.org/uri/RegStatus/1001> ;
    rdfs:domain <http://rdaregistry.info/Elements/c/C10007> ;
    rdfs:isDefinedBy <http://rdaregistry.info/Elements/m/> ;
    rdfs:subPropertyOf <http://rdaregistry.info/Elements/m/P30216> ;
    skos:definition "Relates a manifestation to details of a suspension of light-sensitive chemicals used as a coating on a microfilm or microfiche."@en .

<http://rdaregistry.info/Elements/m/P30224> a rdf:Property ;
    rdfs:label "has details of encoding format"@en,
        "har detaljerad information om kodningsformat"@sv ;
    rdakit:instructionNumber "3.19.3.4" ;
    rdakit:toolkitDefinition "Details of a schema, standard, etc., used to encode the digital content of a manifestation."@en,
        "Detalles del esquema, estándar, etc., utilizado para codificar el contenido digital de un recurso."@es ;
    rdakit:toolkitLabel "details of encoding format"@en,
        "detalles del formato de codificación"@es,
        "detaljerad information om kodningsformat"@sv ;
    reg:hasUnconstrained <http://rdaregistry.info/Elements/u/P60775> ;
    reg:lexicalAlias <http://rdaregistry.info/Elements/m/detailsOfEncodingFormat.en> ;
    reg:name "detailsOfEncodingFormat"@en ;
    reg:status <http://metadataregistry.org/uri/RegStatus/1001> ;
    rdfs:domain <http://rdaregistry.info/Elements/c/C10007> ;
    rdfs:isDefinedBy <http://rdaregistry.info/Elements/m/> ;
    rdfs:subPropertyOf <http://rdaregistry.info/Elements/m/P30221> ;
    skos:definition "Relates a manifestation to details of a schema, standard, etc., used to encode the digital content of a manifestation."@en .

<http://rdaregistry.info/Elements/m/P30225> a rdf:Property ;
    rdfs:label "has details of file type"@en,
        "har detaljerad information om filtyp"@sv ;
    rdakit:instructionNumber "3.19.2.4" ;
    rdakit:toolkitDefinition "Details of a general type of data content encoded in a computer file."@en,
        "Detalles del tipo general de contenido de datos codificado en un archivo de computadora."@es ;
    rdakit:toolkitLabel "details of file type"@en,
        "detalles del tipo de archivo"@es,
        "detaljerad information om filtyp"@sv ;
    reg:hasUnconstrained <http://rdaregistry.info/Elements/u/P60776> ;
    reg:lexicalAlias <http://rdaregistry.info/Elements/m/detailsOfFileType.en> ;
    reg:name "detailsOfFileType"@en ;
    reg:status <http://metadataregistry.org/uri/RegStatus/1001> ;
    rdfs:domain <http://rdaregistry.info/Elements/c/C10007> ;
    rdfs:isDefinedBy <http://rdaregistry.info/Elements/m/> ;
    rdfs:subPropertyOf <http://rdaregistry.info/Elements/m/P30221> ;
    skos:definition "Relates a manifestation to details of a general type of data content encoded in a computer file."@en .

<http://rdaregistry.info/Elements/m/P30232> a rdf:Property ;
    rdfs:label "has details of groove characteristic"@en,
        "har detaljerad information om spårkaraktäristika"@sv ;
    rdakit:instructionNumber "3.16.5.4" ;
    rdakit:toolkitDefinition "Details of a groove width of an analog disc or a groove pitch of an analog cylinder."@en,
        "Detalles de la amplitud del surco de un disco análogo o el tono del surco de un cilindro análogo."@es ;
    rdakit:toolkitLabel "details of groove characteristic"@en,
        "detalles de las características del surco"@es,
        "detaljerad information om spårkaraktäristika"@sv ;
    reg:hasUnconstrained <http://rdaregistry.info/Elements/u/P60783> ;
    reg:lexicalAlias <http://rdaregistry.info/Elements/m/detailsOfGrooveCharacteristic.en> ;
    reg:name "detailsOfGrooveCharacteristic"@en ;
    reg:status <http://metadataregistry.org/uri/RegStatus/1001> ;
    rdfs:domain <http://rdaregistry.info/Elements/c/C10007> ;
    rdfs:isDefinedBy <http://rdaregistry.info/Elements/m/> ;
    rdfs:subPropertyOf <http://rdaregistry.info/Elements/m/P30245> ;
    skos:definition "Relates a manifestation to details of a groove width of an analog disc or a groove pitch of an analog cylinder."@en .

<http://rdaregistry.info/Elements/m/P30241> a rdf:Property ;
    rdfs:label "has details of projection characteristic of motion picture film"@en,
        "har detaljerad information om projektionskarakteristika för film"@sv ;
    rdakit:instructionNumber "3.17.1.4" ;
    rdakit:toolkitDefinition "Details of a technical specification relating to the projection of a motion picture film."@en,
        "Detalles de especificaciones técnicas relacionadas con la proyección de un largometraje."@es ;
    rdakit:toolkitLabel "details of projection characteristic of motion picture film"@en,
        "detalles de características de proyección de un largometraje"@es,
        "detaljerad informatino om projektionskarakteristika för film"@sv ;
    reg:hasSubproperty <http://rdaregistry.info/Elements/m/P30242> ;
    reg:hasUnconstrained <http://rdaregistry.info/Elements/u/P60792> ;
    reg:lexicalAlias <http://rdaregistry.info/Elements/m/detailsOfProjectionCharacteristicOfMotionPictureFilm.en> ;
    reg:name "detailsOfProjectionCharacteristicOfMotionPictureFilm"@en ;
    reg:status <http://metadataregistry.org/uri/RegStatus/1001> ;
    rdfs:domain <http://rdaregistry.info/Elements/c/C10007> ;
    rdfs:isDefinedBy <http://rdaregistry.info/Elements/m/> ;
    skos:definition "Relates a manifestation to details of a technical specification relating to the projection of a motion picture film."@en .

<http://rdaregistry.info/Elements/m/P30242> a rdf:Property ;
    rdfs:label "has details of projection speed"@en,
        "har detaljerad information om projektionshastighet"@sv ;
    rdakit:instructionNumber "3.17.3.4" ;
    rdakit:toolkitDefinition "Details of a speed at which a projected carrier must be operated to produce the moving image intended."@en,
        "Detalles de la velocidad a la cual un proyector debe ser operado para producir la imagen en movimiento esperada."@es ;
    rdakit:toolkitLabel "details of projection speed"@en,
        "detalles de la velocidad de proyección"@es,
        "detaljerad information om projektionshastighet"@sv ;
    reg:hasUnconstrained <http://rdaregistry.info/Elements/u/P60793> ;
    reg:lexicalAlias <http://rdaregistry.info/Elements/m/detailsOfProjectionSpeed.en> ;
    reg:name "detailsOfProjectionSpeed"@en ;
    reg:status <http://metadataregistry.org/uri/RegStatus/1001> ;
    rdfs:domain <http://rdaregistry.info/Elements/c/C10007> ;
    rdfs:isDefinedBy <http://rdaregistry.info/Elements/m/> ;
    rdfs:subPropertyOf <http://rdaregistry.info/Elements/m/P30241> ;
    skos:definition "Relates a manifestation to details of a speed at which a projected carrier must be operated to produce the moving image intended."@en .

<http://rdaregistry.info/Elements/m/P30243> a rdf:Property ;
    rdfs:label "has details of recording medium"@en,
        "har detaljerad information om inspelningssätt"@sv ;
    rdakit:instructionNumber "3.16.3.4" ;
    rdakit:toolkitDefinition "Details of a type of medium used to record sound on an audio carrier ."@en,
        "Detalles del tipo de medio utilizado para grabar el sonido en un soporte de audio (por ej., magnético, óptico)."@es ;
    rdakit:toolkitLabel "details of recording medium"@en,
        "detalles del medio de grabación"@es,
        "detaljerad information om inspelningssätt"@sv ;
    reg:hasUnconstrained <http://rdaregistry.info/Elements/u/P60794> ;
    reg:lexicalAlias <http://rdaregistry.info/Elements/m/detailsOfRecordingMedium.en> ;
    reg:name "detailsOfRecordingMedium"@en ;
    reg:status <http://metadataregistry.org/uri/RegStatus/1001> ;
    rdfs:domain <http://rdaregistry.info/Elements/c/C10007> ;
    rdfs:isDefinedBy <http://rdaregistry.info/Elements/m/> ;
    rdfs:subPropertyOf <http://rdaregistry.info/Elements/m/P30245> ;
    skos:definition "Relates a manifestation to details of a type of medium used to record sound on an audio carrier."@en .

<http://rdaregistry.info/Elements/m/P30246> a rdf:Property ;
    rdfs:label "has details of special playback characteristic"@en,
        "har detaljerad information om specifika uppspelningskaraktäristika"@sv ;
    rdakit:instructionNumber "3.16.9.4" ;
    rdakit:toolkitDefinition "Details of an equalization system, noise reduction system, etc., used in making an audio recording."@en,
        "Detalles de un sistema de ecualización, sistema de reducción del sonido, etc., utilizado en la producción de una grabación de sonido."@es ;
    rdakit:toolkitLabel "details of special playback characteristic"@en,
        "detalles de características especiales de reproducción"@es,
        "detaljerad information om specifika uppspelningskaraktäristika"@sv ;
    reg:hasUnconstrained <http://rdaregistry.info/Elements/u/P60797> ;
    reg:lexicalAlias <http://rdaregistry.info/Elements/m/detailsOfSpecialPlaybackCharacteristic.en> ;
    reg:name "detailsOfSpecialPlaybackCharacteristic"@en ;
    reg:status <http://metadataregistry.org/uri/RegStatus/1001> ;
    rdfs:domain <http://rdaregistry.info/Elements/c/C10007> ;
    rdfs:isDefinedBy <http://rdaregistry.info/Elements/m/> ;
    rdfs:subPropertyOf <http://rdaregistry.info/Elements/m/P30245> ;
    skos:definition "Relates a manifestation to details of an equalization system, noise reduction system, etc., used in making an audio recording."@en .

<http://rdaregistry.info/Elements/m/P30247> a rdf:Property ;
    rdfs:label "has details of tape configuration"@en,
        "har detaljerad information om antal spår"@sv ;
    rdakit:instructionNumber "3.16.7.4" ;
    rdakit:toolkitDefinition "Details of a number of tracks on an audiotape."@en,
        "Detalles del número de pistas en una cinta de audio."@es ;
    rdakit:toolkitLabel "details of tape configuration"@en,
        "detalles de la configuración de cinta"@es,
        "detaljerad information om antal spår"@sv ;
    reg:hasUnconstrained <http://rdaregistry.info/Elements/u/P60798> ;
    reg:lexicalAlias <http://rdaregistry.info/Elements/m/detailsOfTapeConfiguration.en> ;
    reg:name "detailsOfTapeConfiguration"@en ;
    reg:status <http://metadataregistry.org/uri/RegStatus/1001> ;
    rdfs:domain <http://rdaregistry.info/Elements/c/C10007> ;
    rdfs:isDefinedBy <http://rdaregistry.info/Elements/m/> ;
    rdfs:subPropertyOf <http://rdaregistry.info/Elements/m/P30245> ;
    skos:definition "Relates a manifestation to details of a number of tracks on an audiotape."@en .

<http://rdaregistry.info/Elements/m/P30248> a rdf:Property ;
    rdfs:label "has details of track configuration"@en,
        "har detaljerad information om ljudspårskonfiguration för film"@sv ;
    rdakit:instructionNumber "3.16.6.4" ;
    rdakit:toolkitDefinition "Details of a configuration of the audio track on a sound-track film."@en,
        "Detalles de la configuración de la banda de sonido en una película de banda sonora (por ej., pista central)."@es ;
    rdakit:toolkitLabel "details of track configuration"@en,
        "detalles de la configuración de banda sonora"@es,
        "detaljerad information om ljudspårskonfiguration för film"@sv ;
    reg:hasUnconstrained <http://rdaregistry.info/Elements/u/P60799> ;
    reg:lexicalAlias <http://rdaregistry.info/Elements/m/detailsOfTrackConfiguration.en> ;
    reg:name "detailsOfTrackConfiguration"@en ;
    reg:status <http://metadataregistry.org/uri/RegStatus/1001> ;
    rdfs:domain <http://rdaregistry.info/Elements/c/C10007> ;
    rdfs:isDefinedBy <http://rdaregistry.info/Elements/m/> ;
    rdfs:subPropertyOf <http://rdaregistry.info/Elements/m/P30245> ;
    skos:definition "Relates a manifestation to details of a configuration of the audio track on a sound-track film."@en .

<http://rdaregistry.info/Elements/m/P30249> a rdf:Property ;
    rdfs:label "has details of type of recording"@en,
        "har detaljerad information om inspelningstyp"@sv ;
    rdakit:instructionNumber "3.16.2.4" ;
    rdakit:toolkitDefinition "Details of a method used to encode audio content for playback."@en,
        "Detalles del método utilizado para codificar el contenido sonoro para reproducción (por ej., análogo, digital)."@es ;
    rdakit:toolkitLabel "details of type of recording"@en,
        "detalles del tipo de grabación"@es,
        "detaljerad information om inspelningstyp"@sv ;
    reg:hasUnconstrained <http://rdaregistry.info/Elements/u/P60800> ;
    reg:lexicalAlias <http://rdaregistry.info/Elements/m/detailsOfTypeOfRecording.en> ;
    reg:name "detailsOfTypeOfRecording"@en ;
    reg:status <http://metadataregistry.org/uri/RegStatus/1001> ;
    rdfs:domain <http://rdaregistry.info/Elements/c/C10007> ;
    rdfs:isDefinedBy <http://rdaregistry.info/Elements/m/> ;
    rdfs:subPropertyOf <http://rdaregistry.info/Elements/m/P30245> ;
    skos:definition "Relates a manifestation to details of a method used to encode audio content for playback."@en .

<http://rdaregistry.info/Elements/m/P30251> a rdf:Property ;
    rdfs:label "has details of video format"@en,
        "har detaljerad information om videoformat"@sv ;
    rdakit:instructionNumber "3.18.2.4" ;
    rdakit:toolkitDefinition "Details of a standard, etc., used to encode the analog video content of a manifestation."@en,
        "Detalles de la norma, etc., utilizada para codificar el contenido de vídeo análogo de un recurso."@es ;
    rdakit:toolkitLabel "details of video format"@en,
        "detalles del formato de video"@es,
        "detaljerad information om videoformat"@sv ;
    reg:hasUnconstrained <http://rdaregistry.info/Elements/u/P60802> ;
    reg:lexicalAlias <http://rdaregistry.info/Elements/m/detailsOfVideoFormat.en> ;
    reg:name "detailsOfVideoFormat"@en ;
    reg:status <http://metadataregistry.org/uri/RegStatus/1001> ;
    rdfs:domain <http://rdaregistry.info/Elements/c/C10007> ;
    rdfs:isDefinedBy <http://rdaregistry.info/Elements/m/> ;
    rdfs:subPropertyOf <http://rdaregistry.info/Elements/m/P30250> ;
    skos:definition "Relates a manifestation to details of a standard, etc., used to encode the analog video content of a manifestation."@en .

<http://rdaregistry.info/Elements/m/P30253> a rdf:Property ;
    rdfs:label "is subject of (manifestation)"@en ;
    rdakit:toolkitDefinition "A work that is about a manifestation."@en,
        "Una obra que trata sobre la manifestación."@es ;
    rdakit:toolkitLabel "subject of (manifestation)"@en,
        "materia de (manifestación)"@es ;
    reg:hasSubproperty <http://rdaregistry.info/Elements/m/P30254>,
        <http://rdaregistry.info/Elements/m/object/P30253> ;
    reg:hasUnconstrained <http://rdaregistry.info/Elements/u/P60806> ;
    reg:lexicalAlias <http://rdaregistry.info/Elements/m/subjectOfManifestation.en> ;
    reg:name "subjectOfManifestation"@en ;
    reg:status <http://metadataregistry.org/uri/RegStatus/1001> ;
    rdfs:domain <http://rdaregistry.info/Elements/c/C10007> ;
    rdfs:isDefinedBy <http://rdaregistry.info/Elements/m/> ;
    rdfs:subPropertyOf <http://rdaregistry.info/Elements/w/P10283> ;
    skos:definition "Relates a manifestation to a work that is about a manifestation."@en .

<http://rdaregistry.info/Elements/m/P30255> a rdf:Property ;
    rdfs:label "is analysed in (manifestation)"@en,
        "est analysé dans (manifestation)"@fr ;
    rdakit:instructionNumber "23.5" ;
    rdakit:toolkitDefinition "A work that examines a source manifestation to identify its components and their relations."@en,
        "Una obra que examina la manifestación fuente para identificar sus componentes y sus relaciones."@es,
        "Œuvre qui examine la manifestation source pour identifier ses composantes et leurs relations."@fr ;
    rdakit:toolkitLabel "analysed in (manifestation)"@en,
        "analizada en (manifestación)"@es,
        "analysé dans (manifestation)"@fr ;
    reg:hasSubproperty <http://rdaregistry.info/Elements/m/object/P30255> ;
    reg:hasUnconstrained <http://rdaregistry.info/Elements/u/P60219> ;
    reg:lexicalAlias <http://rdaregistry.info/Elements/m/analysedInManifestation.en> ;
    reg:name "analysedInManifestation"@en ;
    reg:status <http://metadataregistry.org/uri/RegStatus/1001> ;
    rdfs:domain <http://rdaregistry.info/Elements/c/C10007> ;
    rdfs:isDefinedBy <http://rdaregistry.info/Elements/m/> ;
    rdfs:subPropertyOf <http://rdaregistry.info/Elements/m/P30254> ;
    skos:definition "Relates a manifestation to a work that examines a source manifestation to identify its components and their relations."@en,
        "Met une manifestation en relation avec une œuvre qui examine la manifestation source pour identifier ses composantes et leurs relations."@fr .

<http://rdaregistry.info/Elements/m/P30256> a rdf:Property ;
    rdfs:label "is commentary in (manifestation)"@en,
        "est le commentaire dans (manifestation)"@fr ;
    rdakit:instructionNumber "23.5" ;
    rdakit:toolkitDefinition "A work that contains a set of explanatory or critical notes on a described manifestation."@en,
        "Una obra que contiene un conjunto de notas explicativas o críticas sobre la manifestación descrita."@es,
        "Œuvre qui contient un ensemble de notes explicatives ou critiques sur la manifestation décrite."@fr ;
    rdakit:toolkitLabel "commentary in (manifestation)"@en,
        "comentario en (manifestación)"@es,
        "commentaire dans (manifestation)"@fr ;
    reg:hasSubproperty <http://rdaregistry.info/Elements/m/object/P30256> ;
    reg:hasUnconstrained <http://rdaregistry.info/Elements/u/P60213> ;
    reg:lexicalAlias <http://rdaregistry.info/Elements/m/commentaryInManifestation.en> ;
    reg:name "commentaryInManifestation"@en ;
    reg:status <http://metadataregistry.org/uri/RegStatus/1001> ;
    rdfs:domain <http://rdaregistry.info/Elements/c/C10007> ;
    rdfs:isDefinedBy <http://rdaregistry.info/Elements/m/> ;
    rdfs:subPropertyOf <http://rdaregistry.info/Elements/m/P30254> ;
    skos:definition "Relates a manifestation to a work that contains a set of explanatory or critical notes on a described manifestation."@en,
        "Met une manifestation en relation avec une œuvre qui contient un ensemble de notes explicatives ou critiques sur la manifestation décrite."@fr .

<http://rdaregistry.info/Elements/m/P30257> a rdf:Property ;
    rdfs:label "is critiqued in (manifestation)"@en,
        "est critiqué dans (manifestation)"@fr ;
    rdakit:instructionNumber "23.5" ;
    rdakit:toolkitDefinition "A work that contains a critical evaluation of a described manifestation."@en,
        "Una obra que contiene una evaluación crítica de la manifestación descrita."@es,
        "Œuvre qui contient une évaluation critique de la manifestation décrite."@fr ;
    rdakit:toolkitLabel "critiqued in (manifestation)"@en,
        "críticada en (manifestación)"@es,
        "critiqué dans (manifestation)"@fr ;
    reg:hasSubproperty <http://rdaregistry.info/Elements/m/object/P30257> ;
    reg:hasUnconstrained <http://rdaregistry.info/Elements/u/P60212> ;
    reg:lexicalAlias <http://rdaregistry.info/Elements/m/critiquedInManifestation.en> ;
    reg:name "critiquedInManifestation"@en ;
    reg:status <http://metadataregistry.org/uri/RegStatus/1001> ;
    rdfs:domain <http://rdaregistry.info/Elements/c/C10007> ;
    rdfs:isDefinedBy <http://rdaregistry.info/Elements/m/> ;
    rdfs:subPropertyOf <http://rdaregistry.info/Elements/m/P30254> ;
    skos:definition "Relates a manifestation to a work that contains a critical evaluation of a described manifestation."@en,
        "Met une manifestation en relation avec une œuvre qui contient une évaluation critique de la manifestation décrite."@fr .

<http://rdaregistry.info/Elements/m/P30258> a rdf:Property ;
    rdfs:label "is evaluated in (manifestation)"@en,
        "est évalué dans (manifestation)"@fr ;
    rdakit:instructionNumber "23.5" ;
    rdakit:toolkitDefinition "A work that examines or judges a described manifestation."@en,
        "Una obra que examina o juzga la manifestación descrita."@es,
        "Œuvre qui examine ou juge la manifestation décrite."@fr ;
    rdakit:toolkitLabel "evaluated in (manifestation)"@en,
        "evaluada en (manifestación)"@es,
        "évalué dans (manifestation)"@fr ;
    reg:hasSubproperty <http://rdaregistry.info/Elements/m/object/P30258> ;
    reg:hasUnconstrained <http://rdaregistry.info/Elements/u/P60218> ;
    reg:lexicalAlias <http://rdaregistry.info/Elements/m/evaluatedInManifestation.en> ;
    reg:name "evaluatedInManifestation"@en ;
    reg:status <http://metadataregistry.org/uri/RegStatus/1001> ;
    rdfs:domain <http://rdaregistry.info/Elements/c/C10007> ;
    rdfs:isDefinedBy <http://rdaregistry.info/Elements/m/> ;
    rdfs:subPropertyOf <http://rdaregistry.info/Elements/m/P30254> ;
    skos:definition "Relates a manifestation to a work that examines or judges a described manifestation."@en,
        "Met une manifestation en relation avec une œuvre qui examine ou juge la manifestation décrite."@fr .

<http://rdaregistry.info/Elements/m/P30259> a rdf:Property ;
    rdfs:label "is reviewed in (manifestation)"@en,
        "est recensé dans (manifestation)"@fr ;
    rdakit:instructionNumber "23.5" ;
    rdakit:toolkitDefinition "A work that contains a brief evaluation of a described manifestation."@en,
        "Una obra que contiene un evaluación breve de la manifestación descrita."@es,
        "Œuvre qui contient une brève évaluation de la manifestation décrite."@fr ;
    rdakit:toolkitLabel "reviewed in (manifestation)"@en,
        "reseñada en (manifestación)"@es,
        "recensé dans (manifestation)"@fr ;
    reg:hasSubproperty <http://rdaregistry.info/Elements/m/object/P30259> ;
    reg:hasUnconstrained <http://rdaregistry.info/Elements/u/P60211> ;
    reg:lexicalAlias <http://rdaregistry.info/Elements/m/reviewedInManifestation.en> ;
    reg:name "reviewedInManifestation"@en ;
    reg:status <http://metadataregistry.org/uri/RegStatus/1001> ;
    rdfs:domain <http://rdaregistry.info/Elements/c/C10007> ;
    rdfs:isDefinedBy <http://rdaregistry.info/Elements/m/> ;
    rdfs:subPropertyOf <http://rdaregistry.info/Elements/m/P30254> ;
    skos:definition "Relates a manifestation to a work that contains a brief evaluation of a described manifestation."@en,
        "Met une manifestation en relation avec une œuvre qui contient une brève évaluation de la manifestation décrite."@fr .

<http://rdaregistry.info/Elements/m/P30260> a rdf:Property ;
    rdfs:label "has note on identifier for manifestation"@en ;
    rdakit:instructionNumber "2.17.14" ;
    rdakit:toolkitDefinition "A note providing information on identifiers for the manifestation not recorded as part of the identifier for a manifestation element."@en ;
    rdakit:toolkitLabel "note on identifier for manifestation"@en ;
    reg:hasUnconstrained <http://rdaregistry.info/Elements/u/P60868> ;
    reg:lexicalAlias <http://rdaregistry.info/Elements/m/noteOnIdentifierForManifestation.en> ;
    reg:name "noteOnIdentifierForManifestation"@en ;
    reg:status <http://metadataregistry.org/uri/RegStatus/1001> ;
    rdfs:domain <http://rdaregistry.info/Elements/c/C10007> ;
    rdfs:isDefinedBy <http://rdaregistry.info/Elements/m/> ;
    rdfs:subPropertyOf <http://rdaregistry.info/Elements/m/P30137> ;
    skos:definition "Relates a manifestation to a note providing information on identifiers for the manifestation not recorded as part of the identifier for a manifestation element."@en .

<http://rdaregistry.info/Elements/m/P30265> a rdf:Property ;
    rdfs:label "has related work (manifestation)"@en ;
    reg:hasSubproperty <http://rdaregistry.info/Elements/m/datatype/P30265>,
        <http://rdaregistry.info/Elements/m/object/P30265> ;
    reg:hasUnconstrained <http://rdaregistry.info/Elements/u/P60313> ;
    reg:lexicalAlias <http://rdaregistry.info/Elements/m/relatedWorkManifestation.en> ;
    reg:name "relatedWorkManifestation"@en ;
    reg:status <http://metadataregistry.org/uri/RegStatus/1001> ;
    rdfs:domain <http://rdaregistry.info/Elements/c/C10007> ;
    rdfs:isDefinedBy <http://rdaregistry.info/Elements/m/> ;
    rdfs:subPropertyOf <http://rdaregistry.info/Elements/m/P30264> ;
    skos:definition "Relates a manifestation to a work associated with a manifestation being described."@en .

<http://rdaregistry.info/Elements/m/P30266> a rdf:Property ;
    rdfs:label "has related expression (manifestation)"@en ;
    reg:hasSubproperty <http://rdaregistry.info/Elements/m/datatype/P30266>,
        <http://rdaregistry.info/Elements/m/object/P30266> ;
    reg:hasUnconstrained <http://rdaregistry.info/Elements/u/P60313> ;
    reg:lexicalAlias <http://rdaregistry.info/Elements/m/relatedExpressionManifestation.en> ;
    reg:name "relatedExpressionManifestation"@en ;
    reg:status <http://metadataregistry.org/uri/RegStatus/1001> ;
    rdfs:domain <http://rdaregistry.info/Elements/c/C10007> ;
    rdfs:isDefinedBy <http://rdaregistry.info/Elements/m/> ;
    rdfs:subPropertyOf <http://rdaregistry.info/Elements/m/P30264> ;
    skos:definition "Relates a manifestation to an expression associated with a manifestation being described."@en .

<http://rdaregistry.info/Elements/m/P30268> a rdf:Property ;
    rdfs:label "has related person (manifestation)"@en ;
    reg:hasSubproperty <http://rdaregistry.info/Elements/m/datatype/P30268>,
        <http://rdaregistry.info/Elements/m/object/P30268> ;
    reg:lexicalAlias <http://rdaregistry.info/Elements/m/relatedPersonManifestation.en> ;
    reg:name "relatedPersonManifestation"@en ;
    reg:status <http://metadataregistry.org/uri/RegStatus/1001> ;
    rdfs:domain <http://rdaregistry.info/Elements/c/C10007> ;
    rdfs:isDefinedBy <http://rdaregistry.info/Elements/m/> ;
    rdfs:subPropertyOf <http://rdaregistry.info/Elements/m/P30267> ;
    skos:definition "Relates a manifestation to a person associated with a manifestation being described."@en .

<http://rdaregistry.info/Elements/m/P30269> a rdf:Property ;
    rdfs:label "has related family (manifestation)"@en ;
    reg:hasSubproperty <http://rdaregistry.info/Elements/m/datatype/P30269>,
        <http://rdaregistry.info/Elements/m/object/P30269> ;
    reg:lexicalAlias <http://rdaregistry.info/Elements/m/relatedFamilyManifestation.en> ;
    reg:name "relatedFamilyManifestation"@en ;
    reg:status <http://metadataregistry.org/uri/RegStatus/1001> ;
    rdfs:domain <http://rdaregistry.info/Elements/c/C10007> ;
    rdfs:isDefinedBy <http://rdaregistry.info/Elements/m/> ;
    rdfs:subPropertyOf <http://rdaregistry.info/Elements/m/P30271> ;
    skos:definition "Relates a manifestation to a family associated with a manifestation being described."@en .

<http://rdaregistry.info/Elements/m/P30270> a rdf:Property ;
    rdfs:label "has related corporate body (manifestation)"@en ;
    reg:hasSubproperty <http://rdaregistry.info/Elements/m/datatype/P30270>,
        <http://rdaregistry.info/Elements/m/object/P30270> ;
    reg:lexicalAlias <http://rdaregistry.info/Elements/m/relatedCorporateBodyManifestation.en> ;
    reg:name "relatedCorporateBodyManifestation"@en ;
    reg:status <http://metadataregistry.org/uri/RegStatus/1001> ;
    rdfs:domain <http://rdaregistry.info/Elements/c/C10007> ;
    rdfs:isDefinedBy <http://rdaregistry.info/Elements/m/> ;
    rdfs:subPropertyOf <http://rdaregistry.info/Elements/m/P30271> ;
    skos:definition "Relates a manifestation to a corporate body associated with a manifestation being described."@en .

<http://rdaregistry.info/Elements/m/P30272> a rdf:Property ;
    rdfs:label "has related place (manifestation)"@en ;
    reg:hasSubproperty <http://rdaregistry.info/Elements/m/datatype/P30272>,
        <http://rdaregistry.info/Elements/m/object/P30272> ;
    reg:lexicalAlias <http://rdaregistry.info/Elements/m/relatedPlaceManifestation.en> ;
    reg:name "relatedPlaceManifestation"@en ;
    reg:status <http://metadataregistry.org/uri/RegStatus/1001> ;
    rdfs:domain <http://rdaregistry.info/Elements/c/C10007> ;
    rdfs:isDefinedBy <http://rdaregistry.info/Elements/m/> ;
    rdfs:subPropertyOf <http://rdaregistry.info/Elements/m/P30264> ;
    skos:definition "Relates a manifestation to a place associated with a manifestation being described."@en .

<http://rdaregistry.info/Elements/m/P30273> a rdf:Property ;
    rdfs:label "has related time-span (manifestation)"@en ;
    reg:hasSubproperty <http://rdaregistry.info/Elements/m/datatype/P30273>,
        <http://rdaregistry.info/Elements/m/object/P30273> ;
    reg:lexicalAlias <http://rdaregistry.info/Elements/m/relatedTimespanManifestation.en> ;
    reg:name "relatedTimespanManifestation"@en ;
    reg:status <http://metadataregistry.org/uri/RegStatus/1001> ;
    rdfs:domain <http://rdaregistry.info/Elements/c/C10007> ;
    rdfs:isDefinedBy <http://rdaregistry.info/Elements/m/> ;
    rdfs:subPropertyOf <http://rdaregistry.info/Elements/m/P30264> ;
    skos:definition "Relates a manifestation to a time-span associated with a manifestation being described."@en .

<http://rdaregistry.info/Elements/m/P30274> a rdf:Property ;
    rdfs:label "has related nomen (manifestation)"@en ;
    reg:hasSubproperty <http://rdaregistry.info/Elements/m/datatype/P30274>,
        <http://rdaregistry.info/Elements/m/object/P30274> ;
    reg:lexicalAlias <http://rdaregistry.info/Elements/m/relatedNomenManifestation.en> ;
    reg:name "relatedNomenManifestation"@en ;
    reg:status <http://metadataregistry.org/uri/RegStatus/1001> ;
    rdfs:domain <http://rdaregistry.info/Elements/c/C10007> ;
    rdfs:isDefinedBy <http://rdaregistry.info/Elements/m/> ;
    rdfs:subPropertyOf <http://rdaregistry.info/Elements/m/P30264> ;
    skos:definition "Relates a manifestation to a nomen associated with a manifestation being described."@en .

<http://rdaregistry.info/Elements/m/P30004> a rdf:Property ;
    rdfs:label "has identifier for manifestation"@en,
        "a pour identifiant de la manifestation"@fr,
        "har identifikator för manifestationen"@sv ;
    rdakit:instructionNumber "2.15" ;
    rdakit:toolkitDefinition "A character string associated with a manifestation that serves to differentiate a manifestation from other manifestations."@en,
        "Una cadena de caracteres asociada con una manifestación que sirve para diferenciar esa manifestación de otras manifestaciones."@es,
        "Chaîne de caractères associée à une manifestation qui sert à distinguer cette manifestation d’autres manifestations."@fr ;
    rdakit:toolkitLabel "identifier for manifestation"@en,
        "identificador de la manifestación"@es,
        "identifiant de la manifestation"@fr,
        "identifikator för manifestationen"@sv ;
    reg:hasSubproperty <http://rdaregistry.info/Elements/m/P30065>,
        <http://rdaregistry.info/Elements/m/P30066> ;
    reg:hasUnconstrained <http://rdaregistry.info/Elements/u/P60052> ;
    reg:lexicalAlias <http://rdaregistry.info/Elements/m/identifierForManifestation.en> ;
    reg:name "identifierForManifestation"@en ;
    reg:status <http://metadataregistry.org/uri/RegStatus/1001> ;
    rdfs:domain <http://rdaregistry.info/Elements/c/C10007> ;
    rdfs:isDefinedBy <http://rdaregistry.info/Elements/m/> ;
    skos:definition "Relates a manifestation to a character string associated with a manifestation that serves to differentiate a manifestation from other manifestations."@en,
        "Met une manifestation en relation avec une chaîne de caractères associée à une manifestation qui sert à distinguer cette manifestation d’autres manifestations."@fr ;
    skos:scopeNote "An identifier for the manifestation includes registered identifiers from internationally recognized schemes, other identifiers assigned by publishers and others following internally devised schemes, identifiers known as fingerprints constructed by combining groups of characters from specified pages of early printed resources, publisher's numbers for notated music, and plate numbers for notated music."@en .

<http://rdaregistry.info/Elements/m/P30027> a rdf:Property ;
    rdfs:label "is accompanied by (manifestation)"@en,
        "est accompagné de (manifestation)"@fr ;
    rdakit:instructionNumber "24.5" ;
    rdakit:toolkitDefinition "A manifestation issued with another manifestation, without any relationship to its content."@en,
        "Una manifestación publicada con otra manifestación, sin ninguna relación con su contenido."@es,
        "Manifestation publiée avec une autre manifestation, sans aucune relation avec son contenu."@fr ;
    rdakit:toolkitLabel "accompanied by (manifestation)"@en,
        "acompañado por (manifestación)"@es,
        "accompagné de (manifestation)"@fr ;
    reg:hasSubproperty <http://rdaregistry.info/Elements/m/P30035>,
        <http://rdaregistry.info/Elements/m/object/P30027> ;
    reg:hasUnconstrained <http://rdaregistry.info/Elements/u/P60196> ;
    reg:lexicalAlias <http://rdaregistry.info/Elements/m/accompaniedByManifestation.en> ;
    reg:name "accompaniedByManifestation"@en ;
    reg:status <http://metadataregistry.org/uri/RegStatus/1001> ;
    rdfs:domain <http://rdaregistry.info/Elements/c/C10007> ;
    rdfs:isDefinedBy <http://rdaregistry.info/Elements/m/> ;
    rdfs:subPropertyOf <http://rdaregistry.info/Elements/m/P30210> ;
    skos:definition "Relates a manifestation to a manifestation issued with another manifestation, without any relationship to its content."@en,
        "Met une manifestation en relation avec une manifestation publiée avec une autre manifestation, sans aucune relation avec son contenu."@fr .

<http://rdaregistry.info/Elements/m/P30031> a rdf:Property ;
    rdfs:label "has facsimile (manifestation)"@en,
        "a pour fac-similé (manifestation)"@fr ;
    rdakit:instructionNumber "24.5" ;
    rdakit:toolkitDefinition "A manifestation that exactly reproduces another manifestation."@en,
        "Una manifestación que reproduce exactamente otra manifestación."@es,
        "Manifestation qui reproduit exactement une autre manifestation."@fr ;
    rdakit:toolkitLabel "facsimile (manifestation)"@en,
        "facsímil (manifestación)"@es,
        "fac-similé (manifestation)"@fr ;
    reg:hasSubproperty <http://rdaregistry.info/Elements/m/P30021>,
        <http://rdaregistry.info/Elements/m/object/P30031> ;
    reg:hasUnconstrained <http://rdaregistry.info/Elements/u/P60217> ;
    reg:lexicalAlias <http://rdaregistry.info/Elements/m/facsimileManifestation.en> ;
    reg:name "facsimileManifestation"@en ;
    reg:status <http://metadataregistry.org/uri/RegStatus/1001> ;
    rdfs:domain <http://rdaregistry.info/Elements/c/C10007> ;
    rdfs:isDefinedBy <http://rdaregistry.info/Elements/m/> ;
    rdfs:subPropertyOf <http://rdaregistry.info/Elements/m/P30039> ;
    skos:definition "Relates a manifestation to a manifestation that exactly reproduces another manifestation."@en,
        "Met une manifestation en relation avec une manifestation qui reproduit exactement une autre manifestation."@fr .

<http://rdaregistry.info/Elements/m/P30047> a rdf:Property ;
    rdfs:label "is facsimile of (manifestation)"@en,
        "est le fac-similé de (manifestation)"@fr ;
    rdakit:instructionNumber "24.5" ;
    rdakit:toolkitDefinition "A manifestation that is used as the basis for an exact reproduction."@en,
        "Una manifestación usada como base para un reproducción exacta."@es,
        "Manifestation servant de base à une reproduction exacte."@fr ;
    rdakit:toolkitLabel "facsimile of (manifestation)"@en,
        "facsímil de (manifestación)"@es,
        "fac-similé de (manifestation)"@fr ;
    reg:hasSubproperty <http://rdaregistry.info/Elements/m/P30045>,
        <http://rdaregistry.info/Elements/m/object/P30047> ;
    reg:hasUnconstrained <http://rdaregistry.info/Elements/u/P60301> ;
    reg:lexicalAlias <http://rdaregistry.info/Elements/m/facsimileOfManifestation.en> ;
    reg:name "facsimileOfManifestation"@en ;
    reg:status <http://metadataregistry.org/uri/RegStatus/1001> ;
    rdfs:domain <http://rdaregistry.info/Elements/c/C10007> ;
    rdfs:isDefinedBy <http://rdaregistry.info/Elements/m/> ;
    rdfs:subPropertyOf <http://rdaregistry.info/Elements/m/P30043> ;
    skos:definition "Relates a manifestation to a manifestation that is used as the basis for an exact reproduction."@en,
        "Met une manifestation en relation avec une manifestation servant de base à une reproduction exacte."@fr .

<http://rdaregistry.info/Elements/m/P30117> a rdf:Property ;
    rdfs:label "has statement of responsibility"@en,
        "a pour mention de responsabilité"@fr,
        "har upphovsuppgift"@sv ;
    rdakit:instructionNumber "2.4" ;
    rdakit:toolkitDefinition "A statement relating to the identification or function of agents responsible for the creation of, or contributing to the realization of, the intellectual or artistic content of a manifestation."@en,
        "Una mención relacionada con la identificación y/o función de personas, familias, o entidades corporativas responsables de la creación de, o que contribuyen a la realización del contenido intelectual del recurso."@es,
        "Mention relative à l’identification et/ou la fonction de toute personne, famille ou collectivité responsable de la création, ou ayant contribué à la réalisation du contenu intellectuel ou artistique d’une ressource."@fr ;
    rdakit:toolkitLabel "statement of responsibility"@en,
        "mención de responsabilidad"@es,
        "mention de responsabilité"@fr,
        "upphovsuppgift"@sv ;
    reg:hasSubproperty <http://rdaregistry.info/Elements/m/P30105>,
        <http://rdaregistry.info/Elements/m/P30116> ;
    reg:hasUnconstrained <http://rdaregistry.info/Elements/u/P60339> ;
    reg:lexicalAlias <http://rdaregistry.info/Elements/m/statementOfResponsibility.en> ;
    reg:name "statementOfResponsibility"@en ;
    reg:status <http://metadataregistry.org/uri/RegStatus/1001> ;
    rdfs:domain <http://rdaregistry.info/Elements/c/C10007> ;
    rdfs:isDefinedBy <http://rdaregistry.info/Elements/m/> ;
    skos:definition "Relates a manifestation to a statement relating to the identification or function of agents responsible for the creation of, or contributing to the realization of, the intellectual or artistic content of a manifestation."@en,
        "Met une manifestation en relation avec une mention relative à l’identification et/ou la fonction de toute personne, famille ou collectivité responsable de la création, ou ayant contribué à la réalisation du contenu intellectuel ou artistique d’une ressource."@fr ;
    skos:scopeNote "A statement of responsibility sometimes includes words or phrases that are neither names nor linking words."@en,
        "Une mention de responsabilité comprend parfois des mots ou des expressions qui ne sont ni des noms ni des mots de liaison."@fr .

<http://rdaregistry.info/Elements/m/P30126> a rdf:Property ;
    rdfs:label "has video characteristic"@en,
        "a pour caractéristique vidéo"@fr,
        "har videokaraktäristika"@sv ;
    rdakit:instructionNumber "3.18" ;
    rdakit:toolkitDefinition "A technical specification relating to the encoding of video images in a manifestation."@en,
        "Una especificación técnica relacionada con la codificación de las imágenes en un recurso."@es,
        "Spécification technique relative à l’encodage des images vidéo d’une ressource."@fr ;
    rdakit:toolkitLabel "video characteristic"@en,
        "características de video"@es,
        "caractéristique vidéo"@fr,
        "videokaraktäristika"@sv ;
    reg:hasSubproperty <http://rdaregistry.info/Elements/m/P30104>,
        <http://rdaregistry.info/Elements/m/P30123> ;
    reg:hasUnconstrained <http://rdaregistry.info/Elements/u/P60352> ;
    reg:lexicalAlias <http://rdaregistry.info/Elements/m/videoCharacteristic.en> ;
    reg:name "videoCharacteristic"@en ;
    reg:status <http://metadataregistry.org/uri/RegStatus/1001> ;
    rdfs:domain <http://rdaregistry.info/Elements/c/C10007> ;
    rdfs:isDefinedBy <http://rdaregistry.info/Elements/m/> ;
    skos:definition "Relates a manifestation to a technical specification relating to the encoding of video images in a manifestation."@en,
        "Met une manifestation en relation avec une spécification technique relative à l’encodage des images vidéo d’une ressource."@fr .

<http://rdaregistry.info/Elements/m/P30127> a rdf:Property ;
    rdfs:label "has projection characteristic of motion picture film"@en,
        "a pour caractéristique de projection d’un film cinématographique"@fr,
        "har projektionskaraktäristika för film"@sv ;
    rdakit:instructionNumber "3.17" ;
    rdakit:toolkitDefinition "A technical specification relating to the projection of a motion picture film."@en,
        "Una especificación técnica relacionada con la proyección de un largometraje."@es,
        "Spécification technique relative à la projection d’un film cinématographique."@fr ;
    rdakit:toolkitLabel "projection characteristic of motion picture film"@en,
        "características de proyección de un largometraje"@es,
        "caractéristique de projection d’un film cinématographique"@fr,
        "projektionskaraktäristika för film"@sv ;
    reg:hasSubproperty <http://rdaregistry.info/Elements/m/P30163>,
        <http://rdaregistry.info/Elements/m/P30200> ;
    reg:hasUnconstrained <http://rdaregistry.info/Elements/u/P60353> ;
    reg:lexicalAlias <http://rdaregistry.info/Elements/m/projectionCharacteristicOfMotionPictureFilm.en> ;
    reg:name "projectionCharacteristicOfMotionPictureFilm"@en ;
    reg:status <http://metadataregistry.org/uri/RegStatus/1001> ;
    rdfs:domain <http://rdaregistry.info/Elements/c/C10007> ;
    rdfs:isDefinedBy <http://rdaregistry.info/Elements/m/> ;
    skos:definition "Relates a manifestation to a technical specification relating to the projection of a motion picture film."@en,
        "Met une manifestation en relation avec une spécification technique relative à la projection d’un film cinématographique."@fr .

<http://rdaregistry.info/Elements/m/P30169> a rdf:Property ;
    rdfs:label "has dimensions"@en,
        "a pour dimensions"@fr,
        "har mått"@sv ;
    rdakit:instructionNumber "3.5" ;
    rdakit:toolkitDefinition "A measurement of a carrier or a container of a manifestation."@en,
        "Las medidas del soporte o soportes y/o el envase de un recurso."@es,
        "Les mesures du ou des supports matériels et/ou du conteneur d’une ressource."@fr ;
    rdakit:toolkitLabel "dimensions"@en,
        "dimensiones"@es,
        "dimensions"@fr,
        "mått"@sv ;
    reg:hasSubproperty <http://rdaregistry.info/Elements/m/P30170>,
        <http://rdaregistry.info/Elements/m/P30171> ;
    reg:hasUnconstrained <http://rdaregistry.info/Elements/u/P60539> ;
    reg:lexicalAlias <http://rdaregistry.info/Elements/m/dimensions.en> ;
    reg:name "dimensions"@en ;
    reg:status <http://metadataregistry.org/uri/RegStatus/1001> ;
    rdfs:domain <http://rdaregistry.info/Elements/c/C10007> ;
    rdfs:isDefinedBy <http://rdaregistry.info/Elements/m/> ;
    skos:definition "Relates a manifestation to a measurement of a carrier or a container of a manifestation."@en,
        "Met une manifestation en relation avec les mesures du ou des supports matériels et/ou du conteneur d’une ressource."@fr ;
    skos:scopeNote "Dimensions include measurements of height, width, depth, length, gauge, and diameter."@en,
        "Les dimensions comprennent les mesures de hauteur, de largeur, de profondeur, de longueur et de diamètre ainsi que le format."@fr .

<http://rdaregistry.info/Elements/m/P30187> a rdf:Property ;
    rdfs:label "has production method"@en,
        "a pour méthode de production"@fr,
        "har produktionsmetod"@sv ;
    rdakit:instructionNumber "3.9" ;
    rdakit:toolkitDefinition "A process used to produce a manifestation."@en,
        "El proceso utilizado para producir un recurso."@es,
        "Le procédé utilisé pour produire une ressource."@fr ;
    rdakit:toolkitLabel "production method"@en,
        "método de producción"@es,
        "méthode de production"@fr,
        "produktionsmetod"@sv ;
    reg:hasSubproperty <http://rdaregistry.info/Elements/m/P30188>,
        <http://rdaregistry.info/Elements/m/P30189> ;
    reg:hasUnconstrained <http://rdaregistry.info/Elements/u/P60560> ;
    reg:lexicalAlias <http://rdaregistry.info/Elements/m/productionMethod.en> ;
    reg:name "productionMethod"@en ;
    reg:status <http://metadataregistry.org/uri/RegStatus/1001> ;
    rdfs:domain <http://rdaregistry.info/Elements/c/C10007> ;
    rdfs:isDefinedBy <http://rdaregistry.info/Elements/m/> ;
    skos:definition "Relates a manifestation to a process used to produce a manifestation."@en,
        "Met une manifestation en relation avec le procédé utilisé pour produire une ressource."@fr .

<http://rdaregistry.info/Elements/m/P30210> a rdf:Property ;
    rdfs:label "has accompanying manifestation relationship with"@en,
        "a pour relation de manifestation d’accompagnement"@fr ;
    rdakit:instructionNumber "24.5" ;
    rdakit:toolkitDefinition "A manifestation that accompanies or is accompanied by another manifestation."@en,
        "Una manifestación que acompaña o está acompañado por la manifestación."@es,
        "Manifestation qui accompagne la manifestation ou est accompagnée par elle."@fr ;
    rdakit:toolkitLabel "accompanying manifestation relationship"@en,
        "relaciones de manifestación acompañante"@es,
        "relation de manifestation d’accompagnement"@fr ;
    reg:hasSubproperty <http://rdaregistry.info/Elements/m/P30027>,
        <http://rdaregistry.info/Elements/m/object/P30210> ;
    reg:hasUnconstrained <http://rdaregistry.info/Elements/u/P60709> ;
    reg:lexicalAlias <http://rdaregistry.info/Elements/m/accompanyingManifestationRelationship.en> ;
    reg:name "accompanyingManifestationRelationship"@en ;
    reg:status <http://metadataregistry.org/uri/RegStatus/1001> ;
    rdfs:domain <http://rdaregistry.info/Elements/c/C10007> ;
    rdfs:isDefinedBy <http://rdaregistry.info/Elements/m/> ;
    rdfs:subPropertyOf <http://rdaregistry.info/Elements/m/P30048> ;
    skos:definition "Relates a manifestation to a manifestation that accompanies or is accompanied by another manifestation."@en,
        "Met une manifestation en relation avec une manifestation qui accompagne la manifestation ou est accompagnée par elle."@fr .

<http://rdaregistry.info/Elements/m/P30212> a rdf:Property ;
    rdfs:label "has equivalent manifestation relationship with"@en,
        "a pour relation de manifestation équivalente"@fr ;
    rdakit:instructionNumber "24.5" ;
    rdakit:toolkitDefinition "A manifestation that is equivalent to another manifestation."@en,
        "Una manifestación que es equivalente a la manifestación."@es,
        "Manifestation qui est équivalente à la manifestation."@fr ;
    rdakit:toolkitLabel "equivalent manifestation relationship"@en,
        "relaciones de manifestación equivalente"@es,
        "relation de manifestation équivalente"@fr ;
    reg:hasSubproperty <http://rdaregistry.info/Elements/m/P30024>,
        <http://rdaregistry.info/Elements/m/object/P30212> ;
    reg:hasUnconstrained <http://rdaregistry.info/Elements/u/P60712> ;
    reg:lexicalAlias <http://rdaregistry.info/Elements/m/equivalentManifestationRelationship.en> ;
    reg:name "equivalentManifestationRelationship"@en ;
    reg:status <http://metadataregistry.org/uri/RegStatus/1001> ;
    rdfs:domain <http://rdaregistry.info/Elements/c/C10007> ;
    rdfs:isDefinedBy <http://rdaregistry.info/Elements/m/> ;
    rdfs:subPropertyOf <http://rdaregistry.info/Elements/m/P30048> ;
    skos:definition "Relates a manifestation to a manifestation that is equivalent to another manifestation."@en,
        "Met une manifestation en relation avec une manifestation qui est équivalente à la manifestation."@fr .

<http://rdaregistry.info/Elements/m/P30250> a rdf:Property ;
    rdfs:label "has details of video characteristic"@en,
        "har detaljerad information om videokaraktäristika"@sv ;
    rdakit:instructionNumber "3.18.1.4" ;
    rdakit:toolkitDefinition "Details of a technical specification relating to the encoding of video images in a manifestation."@en,
        "Detalles de especificaciones técnicas relacionadas con la codificación de las imágenes en un recurso."@es ;
    rdakit:toolkitLabel "details of video characteristic"@en,
        "detalles de características de video"@es,
        "detaljerad information om videokaraktäristika"@sv ;
    reg:hasSubproperty <http://rdaregistry.info/Elements/m/P30219>,
        <http://rdaregistry.info/Elements/m/P30251> ;
    reg:hasUnconstrained <http://rdaregistry.info/Elements/u/P60801> ;
    reg:lexicalAlias <http://rdaregistry.info/Elements/m/detailsOfVideoCharacteristic.en> ;
    reg:name "detailsOfVideoCharacteristic"@en ;
    reg:status <http://metadataregistry.org/uri/RegStatus/1001> ;
    rdfs:domain <http://rdaregistry.info/Elements/c/C10007> ;
    rdfs:isDefinedBy <http://rdaregistry.info/Elements/m/> ;
    skos:definition "Relates a manifestation to details of a technical specification relating to the encoding of video images in a manifestation."@en .

<http://rdaregistry.info/Elements/m/P30035> a rdf:Property ;
    rdfs:label "is issued with"@en,
        "est publié avec"@fr ;
    rdakit:instructionNumber "24.5" ;
    rdakit:toolkitDefinition "A manifestation that is issued on the same carrier as a manifestation being described."@en,
        "Una manifestación que se publica en el mismo soporte que la manifestación que se está describiendo."@es,
        "Manifestation qui est publiée sur le même support matériel que la manifestation décrite."@fr ;
    rdakit:toolkitLabel "issued with"@en,
        "publicado con"@es,
        "publié avec"@fr ;
    reg:hasSubproperty <http://rdaregistry.info/Elements/m/P30036>,
        <http://rdaregistry.info/Elements/m/P30037>,
        <http://rdaregistry.info/Elements/m/object/P30035> ;
    reg:hasUnconstrained <http://rdaregistry.info/Elements/u/P60256> ;
    reg:lexicalAlias <http://rdaregistry.info/Elements/m/issuedWith.en> ;
    reg:name "issuedWith"@en ;
    reg:status <http://metadataregistry.org/uri/RegStatus/1001> ;
    rdfs:domain <http://rdaregistry.info/Elements/c/C10007> ;
    rdfs:isDefinedBy <http://rdaregistry.info/Elements/m/> ;
    rdfs:subPropertyOf <http://rdaregistry.info/Elements/m/P30027> ;
    skos:definition "Relates a manifestation to a manifestation that is issued on the same carrier as a manifestation being described."@en,
        "Met une manifestation en relation avec une manifestation qui est publiée sur le même support matériel que la manifestation décrite."@fr .

<http://rdaregistry.info/Elements/m/P30156> a rdf:Property ;
    rdfs:label "has title proper"@en,
        "a pour titre propre"@fr,
        "har huvudtitel"@sv ;
    rdakit:instructionNumber "2.3.2" ;
    rdakit:toolkitDefinition "A chief name of a manifestation, that is, a title normally used when naming a manifestation."@en,
        "El nombre principal de un recurso (i.e., el título normalmente usado para citar el recurso)."@es,
        "Le titre principal d’une ressource (c’est-à-dire le titre normalement utilisé pour citer la ressource)."@fr ;
    rdakit:toolkitLabel "title proper"@en,
        "título propiamente dicho"@es,
        "titre propre"@fr,
        "huvudtitel"@sv ;
    reg:hasUnconstrained <http://rdaregistry.info/Elements/u/P60515> ;
    reg:lexicalAlias <http://rdaregistry.info/Elements/m/titleProper.en> ;
    reg:name "titleProper"@en ;
    reg:status <http://metadataregistry.org/uri/RegStatus/1001> ;
    rdfs:domain <http://rdaregistry.info/Elements/c/C10007> ;
    rdfs:isDefinedBy <http://rdaregistry.info/Elements/m/> ;
    rdfs:subPropertyOf <http://rdaregistry.info/Elements/m/P30134> ;
    skos:definition "Relates a manifestation to a chief name of a manifestation, that is, a title normally used when naming a manifestation."@en,
        "Met une manifestation en relation avec le titre principal d’une ressource (c’est-à-dire le titre normalement utilisé pour citer la ressource)."@fr ;
    skos:scopeNote "An alternative title is treated as part of a title proper."@en .

<http://rdaregistry.info/Elements/m/P30213> a rdf:Property ;
    rdfs:label "has whole-part manifestation relationship with"@en,
        "a pour relation de manifestation tout-partie"@fr ;
    rdakit:instructionNumber "24.5" ;
    rdakit:toolkitDefinition "A manifestation that is contained in or contains another manifestation."@en,
        "Una manifestación que está incluida en, o contiene la manifestación."@es,
        "Manifestation qui est contenue dans la manifestation ou la contient."@fr ;
    rdakit:toolkitLabel "whole-part manifestation relationship"@en,
        "relación de la manifestación todo-parte"@es,
        "relation de manifestation tout-partie"@fr ;
    reg:hasSubproperty <http://rdaregistry.info/Elements/m/P30020>,
        <http://rdaregistry.info/Elements/m/P30033>,
        <http://rdaregistry.info/Elements/m/object/P30213> ;
    reg:hasUnconstrained <http://rdaregistry.info/Elements/u/P60714> ;
    reg:lexicalAlias <http://rdaregistry.info/Elements/m/wholePartManifestationRelationship.en> ;
    reg:name "wholePartManifestationRelationship"@en ;
    reg:status <http://metadataregistry.org/uri/RegStatus/1001> ;
    rdfs:domain <http://rdaregistry.info/Elements/c/C10007> ;
    rdfs:isDefinedBy <http://rdaregistry.info/Elements/m/> ;
    rdfs:subPropertyOf <http://rdaregistry.info/Elements/m/P30048> ;
    skos:definition "Relates a manifestation to a manifestation that is contained in or contains another manifestation."@en,
        "Met une manifestation en relation avec une manifestation qui est contenue dans la manifestation ou la contient."@fr .

<http://rdaregistry.info/Elements/m/P30214> a rdf:Property ;
    rdfs:label "has note on carrier"@en,
        "a pour note sur le support matériel"@fr,
        "har anmärkning om bärare"@sv ;
    rdakit:instructionNumber "3.21" ;
    rdakit:toolkitDefinition "A note providing information on attributes of a carrier or carriers of a manifestation."@en,
        "Una nota que proporciona información sobre los atributos del soporte o soportes de la manifestación."@es,
        "Note fournissant de l’information sur les attributs du ou des supports matériels de la manifestation."@fr ;
    rdakit:toolkitLabel "note on carrier"@en,
        "nota sobre el soporte"@es,
        "note sur le support matériel"@fr,
        "anmärkning om bärare"@sv ;
    reg:hasSubproperty <http://rdaregistry.info/Elements/m/P30060>,
        <http://rdaregistry.info/Elements/m/P30061> ;
    reg:hasUnconstrained <http://rdaregistry.info/Elements/u/P60470> ;
    reg:lexicalAlias <http://rdaregistry.info/Elements/m/noteOnCarrier.en> ;
    reg:name "noteOnCarrier"@en ;
    reg:status <http://metadataregistry.org/uri/RegStatus/1001> ;
    rdfs:domain <http://rdaregistry.info/Elements/c/C10007> ;
    rdfs:isDefinedBy <http://rdaregistry.info/Elements/m/> ;
    skos:definition "Relates a manifestation to a note providing information on attributes of a carrier or carriers of a manifestation."@en,
        "Met une manifestation en relation avec une note fournissant de l’information sur les attributs du ou des supports matériels de la manifestation."@fr .

<http://rdaregistry.info/Elements/m/P30271> a rdf:Property ;
    rdfs:label "has related collective agent (manifestation)"@en ;
    reg:hasSubproperty <http://rdaregistry.info/Elements/m/P30269>,
        <http://rdaregistry.info/Elements/m/P30270>,
        <http://rdaregistry.info/Elements/m/datatype/P30271>,
        <http://rdaregistry.info/Elements/m/object/P30271> ;
    reg:lexicalAlias <http://rdaregistry.info/Elements/m/relatedCollectiveAgentManifestation.en> ;
    reg:name "relatedCollectiveAgentManifestation"@en ;
    reg:status <http://metadataregistry.org/uri/RegStatus/1001> ;
    rdfs:domain <http://rdaregistry.info/Elements/c/C10007> ;
    rdfs:isDefinedBy <http://rdaregistry.info/Elements/m/> ;
    rdfs:subPropertyOf <http://rdaregistry.info/Elements/m/P30267> ;
    skos:definition "Relates a manifestation to a collective agent associated with a manifestation being described."@en .

<http://rdaregistry.info/Elements/m/P30020> a rdf:Property ;
    rdfs:label "is contained in (manifestation)"@en,
        "est contenu dans (manifestation)"@fr ;
    rdakit:instructionNumber "24.5" ;
    rdakit:toolkitDefinition "A larger manifestation of which the manifestation is a discrete component."@en,
        "Una manifestación mayor de la cual una parte es un componente separado."@es,
        "Manifestation plus vaste dont la manifestation est une composante distincte."@fr ;
    rdakit:toolkitLabel "contained in (manifestation)"@en,
        "contenida en (manifestación)"@es,
        "contenu dans (manifestation)"@fr ;
    reg:hasSubproperty <http://rdaregistry.info/Elements/m/P30019>,
        <http://rdaregistry.info/Elements/m/P30025>,
        <http://rdaregistry.info/Elements/m/P30101>,
        <http://rdaregistry.info/Elements/m/object/P30020> ;
    reg:hasUnconstrained <http://rdaregistry.info/Elements/u/P60101> ;
    reg:lexicalAlias <http://rdaregistry.info/Elements/m/containedInManifestation.en> ;
    reg:name "containedInManifestation"@en ;
    reg:status <http://metadataregistry.org/uri/RegStatus/1001> ;
    rdfs:domain <http://rdaregistry.info/Elements/c/C10007> ;
    rdfs:isDefinedBy <http://rdaregistry.info/Elements/m/> ;
    rdfs:subPropertyOf <http://rdaregistry.info/Elements/m/P30213> ;
    skos:definition "Relates a manifestation to a larger manifestation of which the manifestation is a discrete component."@en,
        "Met une manifestation en relation avec une manifestation plus vaste dont la manifestation est une composante distincte."@fr .

<http://rdaregistry.info/Elements/m/P30033> a rdf:Property ;
    rdfs:label "is container of (manifestation)"@en,
        "est le conteneur de (manifestation)"@fr ;
    rdakit:instructionNumber "24.5" ;
    rdakit:toolkitDefinition "A manifestation that is a discrete component of a larger manifestation."@en,
        "Una manifestación que es un componente separado de una entidad mayor."@es,
        "Manifestation qui est une composante distincte d’une manifestation plus vaste."@fr ;
    rdakit:toolkitLabel "container of (manifestation)"@en,
        "contiene (manifestación)"@es,
        "conteneur de (manifestation)"@fr ;
    reg:hasSubproperty <http://rdaregistry.info/Elements/m/P30022>,
        <http://rdaregistry.info/Elements/m/P30030>,
        <http://rdaregistry.info/Elements/m/P30046>,
        <http://rdaregistry.info/Elements/m/object/P30033> ;
    reg:hasUnconstrained <http://rdaregistry.info/Elements/u/P60249> ;
    reg:lexicalAlias <http://rdaregistry.info/Elements/m/containerOfManifestation.en> ;
    reg:name "containerOfManifestation"@en ;
    reg:status <http://metadataregistry.org/uri/RegStatus/1001> ;
    rdfs:domain <http://rdaregistry.info/Elements/c/C10007> ;
    rdfs:isDefinedBy <http://rdaregistry.info/Elements/m/> ;
    rdfs:subPropertyOf <http://rdaregistry.info/Elements/m/P30213> ;
    skos:definition "Relates a manifestation to a manifestation that is a discrete component of a larger manifestation."@en,
        "Met une manifestation en relation avec une manifestation qui est une composante distincte d’une manifestation plus vaste."@fr .

<http://rdaregistry.info/Elements/m/P30048> a rdf:Property ;
    rdfs:label "has related manifestation (manifestation)"@en,
        "har relaterad manifestation"@sv ;
    rdakit:toolkitLabel "relaterad manifestation"@sv ;
    reg:hasSubproperty <http://rdaregistry.info/Elements/m/P30210>,
        <http://rdaregistry.info/Elements/m/P30212>,
        <http://rdaregistry.info/Elements/m/P30213>,
        <http://rdaregistry.info/Elements/m/datatype/P30048>,
        <http://rdaregistry.info/Elements/m/object/P30048> ;
    reg:hasUnconstrained <http://rdaregistry.info/Elements/u/P60313> ;
    reg:lexicalAlias <http://rdaregistry.info/Elements/m/relatedManifestationManifestation.en> ;
    reg:name "relatedManifestationManifestation"@en ;
    reg:status <http://metadataregistry.org/uri/RegStatus/1001> ;
    rdfs:domain <http://rdaregistry.info/Elements/c/C10007> ;
    rdfs:isDefinedBy <http://rdaregistry.info/Elements/m/> ;
    rdfs:subPropertyOf <http://rdaregistry.info/Elements/m/P30264> ;
    skos:definition "Relates a manifestation to a manifestation associated with a manifestation being described."@en .

<http://rdaregistry.info/Elements/m/P30221> a rdf:Property ;
    rdfs:label "has details of digital file characteristic"@en,
        "har detaljerad information om egenskaper för resursens digitala kodning"@sv ;
    rdakit:instructionNumber "3.19.1.4" ;
    rdakit:toolkitDefinition "Details of a technical specification relating to the digital encoding of text, image, audio, video, and other types of data in a manifestation."@en,
        "Detalles de especificaciones técnicas relacionadas con la codificación digital de un texto, imagen, audio, vídeo y otros tipos de datos en un recurso."@es ;
    rdakit:toolkitLabel "details of digital file characteristic"@en,
        "detalles de las características del archivo digital"@es,
        "detaljerad information om egenskaper för resursens digitala kodning"@sv ;
    reg:hasSubproperty <http://rdaregistry.info/Elements/m/P30222>,
        <http://rdaregistry.info/Elements/m/P30224>,
        <http://rdaregistry.info/Elements/m/P30225> ;
    reg:hasUnconstrained <http://rdaregistry.info/Elements/u/P60772> ;
    reg:lexicalAlias <http://rdaregistry.info/Elements/m/detailsOfDigitalFileCharacteristic.en> ;
    reg:name "detailsOfDigitalFileCharacteristic"@en ;
    reg:status <http://metadataregistry.org/uri/RegStatus/1001> ;
    rdfs:domain <http://rdaregistry.info/Elements/c/C10007> ;
    rdfs:isDefinedBy <http://rdaregistry.info/Elements/m/> ;
    skos:definition "Relates a manifestation to details of a technical specification relating to the digital encoding of text, image, audio, video, and other types of data in a manifestation."@en .

<http://rdaregistry.info/Elements/m/P30024> a rdf:Property ;
    rdfs:label "has equivalent (manifestation)"@en,
        "est l’équivalent (manifestation)"@fr ;
    rdakit:instructionNumber "24.5" ;
    rdakit:toolkitDefinition "A manifestation that embodies the same expression of a work."@en,
        "Una manifestación que materializa la misma expresión de una obra."@es,
        "Manifestation qui matérialise la même expression d’une œuvre."@fr ;
    rdakit:toolkitLabel "equivalent (manifestation)"@en,
        "equivalente (manifestación)"@es,
        "équivalent (manifestation)"@fr ;
    reg:hasSubproperty <http://rdaregistry.info/Elements/m/P30026>,
        <http://rdaregistry.info/Elements/m/P30028>,
        <http://rdaregistry.info/Elements/m/P30039>,
        <http://rdaregistry.info/Elements/m/P30043>,
        <http://rdaregistry.info/Elements/m/object/P30024> ;
    reg:hasUnconstrained <http://rdaregistry.info/Elements/u/P60191> ;
    reg:lexicalAlias <http://rdaregistry.info/Elements/m/equivalentManifestation.en> ;
    reg:name "equivalentManifestation"@en ;
    reg:status <http://metadataregistry.org/uri/RegStatus/1001> ;
    rdfs:domain <http://rdaregistry.info/Elements/c/C10007> ;
    rdfs:isDefinedBy <http://rdaregistry.info/Elements/m/> ;
    rdfs:subPropertyOf <http://rdaregistry.info/Elements/m/P30212> ;
    skos:definition "Relates a manifestation to a manifestation that embodies the same expression of a work."@en,
        "Met une manifestation en relation avec une manifestation qui matérialise la même expression d’une œuvre."@fr .

<http://rdaregistry.info/Elements/m/P30039> a rdf:Property ;
    rdfs:label "is reproduced as (manifestation)"@en,
        "est reproduit comme (manifestation)"@fr ;
    rdakit:instructionNumber "24.5" ;
    rdakit:toolkitDefinition "A manifestation that reproduces another manifestation."@en,
        "Una manifestación que reproduce otra manifestación."@es,
        "Manifestation qui reproduit une autre manifestation."@fr ;
    rdakit:toolkitLabel "reproduced as (manifestation)"@en,
        "reproducida como (manifestación)"@es,
        "reproduit comme (manifestation)"@fr ;
    reg:hasSubproperty <http://rdaregistry.info/Elements/m/P30016>,
        <http://rdaregistry.info/Elements/m/P30029>,
        <http://rdaregistry.info/Elements/m/P30031>,
        <http://rdaregistry.info/Elements/m/P30038>,
        <http://rdaregistry.info/Elements/m/object/P30039> ;
    reg:hasUnconstrained <http://rdaregistry.info/Elements/u/P60272> ;
    reg:lexicalAlias <http://rdaregistry.info/Elements/m/reproducedAsManifestation.en> ;
    reg:name "reproducedAsManifestation"@en ;
    reg:status <http://metadataregistry.org/uri/RegStatus/1001> ;
    rdfs:domain <http://rdaregistry.info/Elements/c/C10007> ;
    rdfs:isDefinedBy <http://rdaregistry.info/Elements/m/> ;
    rdfs:subPropertyOf <http://rdaregistry.info/Elements/m/P30024> ;
    skos:definition "Relates a manifestation to a manifestation that reproduces another manifestation."@en,
        "Met une manifestation en relation avec une manifestation qui reproduit une autre manifestation."@fr .

<http://rdaregistry.info/Elements/m/P30043> a rdf:Property ;
    rdfs:label "is reproduction of (manifestation)"@en,
        "est la reproduction de (manifestation)"@fr ;
    rdakit:instructionNumber "24.5" ;
    rdakit:toolkitDefinition "A manifestation that is used as the basis for a reproduction."@en,
        "Una manifestación utilizada como base para una reproducción."@es,
        "Manifestation servant de base à une reproduction."@fr ;
    rdakit:toolkitLabel "reproduction of (manifestation)"@en,
        "reproducción de (manifestación)"@es,
        "reproduction de (manifestation)"@fr ;
    reg:hasSubproperty <http://rdaregistry.info/Elements/m/P30040>,
        <http://rdaregistry.info/Elements/m/P30047>,
        <http://rdaregistry.info/Elements/m/P30093>,
        <http://rdaregistry.info/Elements/m/P30136>,
        <http://rdaregistry.info/Elements/m/object/P30043> ;
    reg:hasUnconstrained <http://rdaregistry.info/Elements/u/P60297> ;
    reg:lexicalAlias <http://rdaregistry.info/Elements/m/reproductionOfManifestation.en> ;
    reg:name "reproductionOfManifestation"@en ;
    reg:status <http://metadataregistry.org/uri/RegStatus/1001> ;
    rdfs:domain <http://rdaregistry.info/Elements/c/C10007> ;
    rdfs:isDefinedBy <http://rdaregistry.info/Elements/m/> ;
    rdfs:subPropertyOf <http://rdaregistry.info/Elements/m/P30024> ;
    skos:definition "Relates a manifestation to a manifestation that is used as the basis for a reproduction."@en,
        "Met une manifestation en relation avec une manifestation servant de base à une reproduction."@fr .

<http://rdaregistry.info/Elements/m/P30182> a rdf:Property ;
    rdfs:label "has extent"@en,
        "a pour importance matérielle"@fr,
        "har omfång"@sv ;
    rdakit:instructionNumber "3.4" ;
    rdakit:toolkitDefinition "A number and type of unit and/or subunit of a manifestation."@en,
        "El número y tipo de unidades y/o subunidades que constituyen un recurso."@es,
        "Le nombre et le type d’unités et/ou de sous-unités formant une ressource."@fr ;
    rdakit:toolkitLabel "extent"@en,
        "extensión"@es,
        "importance matérielle"@fr,
        "omfång"@sv ;
    reg:hasSubproperty <http://rdaregistry.info/Elements/m/P30177>,
        <http://rdaregistry.info/Elements/m/P30178>,
        <http://rdaregistry.info/Elements/m/P30179>,
        <http://rdaregistry.info/Elements/m/P30180>,
        <http://rdaregistry.info/Elements/m/P30181> ;
    reg:hasUnconstrained <http://rdaregistry.info/Elements/u/P60550> ;
    reg:lexicalAlias <http://rdaregistry.info/Elements/m/extent.en> ;
    reg:name "extent"@en ;
    reg:status <http://metadataregistry.org/uri/RegStatus/1001> ;
    rdfs:domain <http://rdaregistry.info/Elements/c/C10007> ;
    rdfs:isDefinedBy <http://rdaregistry.info/Elements/m/> ;
    skos:definition "Relates a manifestation to a number and type of unit or subunit of a manifestation."@en,
        "Met une manifestation en relation avec le nombre et le type d’unités et/ou de sous-unités formant une ressource."@fr .

<http://rdaregistry.info/Elements/m/P30191> a rdf:Property ;
    rdfs:label "has generation"@en,
        "a pour génération"@fr,
        "har generation"@sv ;
    rdakit:instructionNumber "3.10" ;
    rdakit:toolkitDefinition "A relationship between an original carrier and the carrier of a reproduction made from the original."@en,
        "La relación entre un soporte original y el soporte de una reproducción del original (por ej., una cámara maestra de primera generación, una impresión maestra de segunda generación)."@es,
        "La relation entre un support matériel original et le support matériel d’une reproduction faite à partir de l’original (par exemple, un microfilm de prise de vue (première génération), une matrice (deuxième génération))."@fr ;
    rdakit:toolkitLabel "generation"@en,
        "generación"@es,
        "génération"@fr,
        "generation"@sv ;
    reg:hasSubproperty <http://rdaregistry.info/Elements/m/P30190>,
        <http://rdaregistry.info/Elements/m/P30192>,
        <http://rdaregistry.info/Elements/m/P30193>,
        <http://rdaregistry.info/Elements/m/P30194>,
        <http://rdaregistry.info/Elements/m/P30195> ;
    reg:hasUnconstrained <http://rdaregistry.info/Elements/u/P60568> ;
    reg:lexicalAlias <http://rdaregistry.info/Elements/m/generation.en> ;
    reg:name "generation"@en ;
    reg:status <http://metadataregistry.org/uri/RegStatus/1001> ;
    rdfs:domain <http://rdaregistry.info/Elements/c/C10007> ;
    rdfs:isDefinedBy <http://rdaregistry.info/Elements/m/> ;
    skos:definition "Relates a manifestation to a relationship between an original carrier and the carrier of a reproduction made from the original."@en,
        "Met une manifestation en relation avec la relation entre un support matériel original et le support matériel d’une reproduction faite à partir de l’original (par exemple, un microfilm de prise de vue (première génération), une matrice (deuxième génération))."@fr .

<http://rdaregistry.info/Elements/m/P30254> a rdf:Property ;
    rdfs:label "is described in (manifestation)"@en,
        "est décrit dans (manifestation)"@fr ;
    rdakit:instructionNumber "23.5" ;
    rdakit:toolkitDefinition "A work that describes a described manifestation."@en,
        "Una obra que describe una manifestación descrita."@es,
        "Œuvre qui décrit une manifestation décrite."@fr ;
    rdakit:toolkitLabel "described in (manifestation)"@en,
        "descrita en (manifestación)"@es,
        "décrit dans (manifestation)"@fr ;
    reg:hasSubproperty <http://rdaregistry.info/Elements/m/P30255>,
        <http://rdaregistry.info/Elements/m/P30256>,
        <http://rdaregistry.info/Elements/m/P30257>,
        <http://rdaregistry.info/Elements/m/P30258>,
        <http://rdaregistry.info/Elements/m/P30259>,
        <http://rdaregistry.info/Elements/m/object/P30254> ;
    reg:hasUnconstrained <http://rdaregistry.info/Elements/u/P60215> ;
    reg:lexicalAlias <http://rdaregistry.info/Elements/m/describedInManifestation.en> ;
    reg:name "describedInManifestation"@en ;
    reg:status <http://metadataregistry.org/uri/RegStatus/1001> ;
    rdfs:domain <http://rdaregistry.info/Elements/c/C10007> ;
    rdfs:isDefinedBy <http://rdaregistry.info/Elements/m/> ;
    rdfs:subPropertyOf <http://rdaregistry.info/Elements/m/P30253> ;
    skos:definition "Relates a manifestation to a work that describes a described manifestation."@en,
        "Met une manifestation en relation avec une œuvre qui décrit une manifestation décrite."@fr .

<http://rdaregistry.info/Elements/m/P30124> a rdf:Property ;
    rdfs:label "has digital file characteristic"@en,
        "a pour caractéristique du fichier numérique"@fr,
        "har egenskaper för resursens digitala kodning"@sv ;
    rdakit:instructionNumber "3.19" ;
    rdakit:toolkitDefinition "A technical specification relating to the digital encoding of text, image, audio, video, and other types of data in a manifestation."@en,
        "Una especificación técnica relacionada con la codificación digital de un texto, imagen, audio, vídeo y otros tipos de datos en un recurso."@es,
        "Spécification technique relative à l’encodage numérique de texte, d’image, de données audio, vidéo et autres types de données dans une ressource."@fr ;
    rdakit:toolkitLabel "digital file characteristic"@en,
        "características del archivo digital"@es,
        "caractéristique du fichier numérique"@fr,
        "egenskaper för resursens digitala kodning"@sv ;
    reg:hasSubproperty <http://rdaregistry.info/Elements/m/P30006>,
        <http://rdaregistry.info/Elements/m/P30018>,
        <http://rdaregistry.info/Elements/m/P30096>,
        <http://rdaregistry.info/Elements/m/P30102>,
        <http://rdaregistry.info/Elements/m/P30159>,
        <http://rdaregistry.info/Elements/m/P30183>,
        <http://rdaregistry.info/Elements/m/P30202> ;
    reg:hasUnconstrained <http://rdaregistry.info/Elements/u/P60350> ;
    reg:lexicalAlias <http://rdaregistry.info/Elements/m/digitalFileCharacteristic.en> ;
    reg:name "digitalFileCharacteristic"@en ;
    reg:status <http://metadataregistry.org/uri/RegStatus/1001> ;
    rdfs:domain <http://rdaregistry.info/Elements/c/C10007> ;
    rdfs:isDefinedBy <http://rdaregistry.info/Elements/m/> ;
    skos:definition "Relates a manifestation to a technical specification relating to the digital encoding of text, image, audio, video, and other types of data in a manifestation."@en,
        "Met une manifestation en relation avec une spécification technique relative à l’encodage numérique de texte, d’image, de données audio, vidéo et autres types de données dans une ressource."@fr .

<http://rdaregistry.info/Elements/m/P30134> a rdf:Property ;
    rdfs:label "has title"@en,
        "a pour titre"@fr,
        "har titel"@sv ;
    rdakit:instructionNumber "2.3" ;
    rdakit:toolkitDefinition "A word, character, or group of words or characters that names a manifestation or a work embodied in it."@en,
        "Una palabra, carácter, o un grupo de palabras y/o caracteres que nombran un recurso o una obra contenida en ella."@es,
        "Mot, caractère ou groupe de mots et/ou de caractères qui nomme une ressource ou une œuvre contenue dans cette ressource."@fr ;
    rdakit:toolkitLabel "title"@en,
        "título"@es,
        "titre"@fr,
        "titel"@sv ;
    reg:hasSubproperty <http://rdaregistry.info/Elements/m/P30128>,
        <http://rdaregistry.info/Elements/m/P30131>,
        <http://rdaregistry.info/Elements/m/P30142>,
        <http://rdaregistry.info/Elements/m/P30151>,
        <http://rdaregistry.info/Elements/m/P30156>,
        <http://rdaregistry.info/Elements/m/P30203>,
        <http://rdaregistry.info/Elements/m/P30209> ;
    reg:hasUnconstrained <http://rdaregistry.info/Elements/u/P60369> ;
    reg:lexicalAlias <http://rdaregistry.info/Elements/m/title.en> ;
    reg:name "title"@en ;
    reg:status <http://metadataregistry.org/uri/RegStatus/1001> ;
    rdfs:domain <http://rdaregistry.info/Elements/c/C10007> ;
    rdfs:isDefinedBy <http://rdaregistry.info/Elements/m/> ;
    skos:definition "Relates a manifestation to a word, character, or group of words or characters that names a manifestation or a work embodied in it."@en,
        "Met une manifestation en relation avec un mot, un caractère ou un groupe de mots et/ou de caractères qui nomme une ressource ou une œuvre contenue dans cette ressource."@fr .

<http://rdaregistry.info/Elements/m/P30245> a rdf:Property ;
    rdfs:label "has details of sound characteristic"@en,
        "har detaljerad information om ljudkaraktäristika"@sv ;
    rdakit:instructionNumber "3.16.1.4" ;
    rdakit:toolkitDefinition "Details of a technical specification relating to the encoding of sound in a manifestation."@en,
        "Detalles de especificaciones técnicas relacionadas con la codificación del sonido en un recurso."@es ;
    rdakit:toolkitLabel "details of sound characteristic"@en,
        "detalles de las características de sonido"@es,
        "detaljerad information om ljudkaraktäristika"@sv ;
    reg:hasSubproperty <http://rdaregistry.info/Elements/m/P30220>,
        <http://rdaregistry.info/Elements/m/P30232>,
        <http://rdaregistry.info/Elements/m/P30243>,
        <http://rdaregistry.info/Elements/m/P30246>,
        <http://rdaregistry.info/Elements/m/P30247>,
        <http://rdaregistry.info/Elements/m/P30248>,
        <http://rdaregistry.info/Elements/m/P30249> ;
    reg:hasUnconstrained <http://rdaregistry.info/Elements/u/P60796> ;
    reg:lexicalAlias <http://rdaregistry.info/Elements/m/detailsOfSoundCharacteristic.en> ;
    reg:name "detailsOfSoundCharacteristic"@en ;
    reg:status <http://metadataregistry.org/uri/RegStatus/1001> ;
    rdfs:domain <http://rdaregistry.info/Elements/c/C10007> ;
    rdfs:isDefinedBy <http://rdaregistry.info/Elements/m/> ;
    skos:definition "Relates a manifestation to details of a technical specification relating to the encoding of sound in a manifestation."@en .

<http://rdaregistry.info/Elements/m/P30125> a rdf:Property ;
    rdfs:label "has sound characteristic"@en,
        "a pour caractéristique sonore"@fr,
        "har ljudkaraktäristiska"@sv ;
    rdakit:instructionNumber "3.16" ;
    rdakit:toolkitDefinition "A technical specification relating to the encoding of sound in a manifestation."@en,
        "Una especificación técnica relacionada con la codificación del sonido en un recurso."@es,
        "Spécification technique relative à l’encodage du son dans une ressource."@fr ;
    rdakit:toolkitLabel "sound characteristic"@en,
        "características de sonido"@es,
        "caractéristique sonore"@fr,
        "ljudkaraktäristiska"@sv ;
    reg:hasSubproperty <http://rdaregistry.info/Elements/m/P30138>,
        <http://rdaregistry.info/Elements/m/P30161>,
        <http://rdaregistry.info/Elements/m/P30164>,
        <http://rdaregistry.info/Elements/m/P30172>,
        <http://rdaregistry.info/Elements/m/P30184>,
        <http://rdaregistry.info/Elements/m/P30185>,
        <http://rdaregistry.info/Elements/m/P30201>,
        <http://rdaregistry.info/Elements/m/P30206> ;
    reg:hasUnconstrained <http://rdaregistry.info/Elements/u/P60351> ;
    reg:lexicalAlias <http://rdaregistry.info/Elements/m/soundCharacteristic.en> ;
    reg:name "soundCharacteristic"@en ;
    reg:status <http://metadataregistry.org/uri/RegStatus/1001> ;
    rdfs:domain <http://rdaregistry.info/Elements/c/C10007> ;
    rdfs:isDefinedBy <http://rdaregistry.info/Elements/m/> ;
    skos:definition "Relates a manifestation to a technical specification relating to the encoding of sound in a manifestation."@en,
        "Met une manifestation en relation avec une spécification technique relative à l’encodage du son dans une ressource."@fr .

<http://rdaregistry.info/Elements/m/P30165> a rdf:Property ;
    rdfs:label "has numbering of serials"@en,
        "a pour numérotation des publications en série"@fr,
        "har numrering av seriella resurser"@sv ;
    rdakit:instructionNumber "2.6" ;
    rdakit:toolkitDefinition "A designation for each of the issues or parts of a serial."@en,
        "La identificación de cada una de las entregas o partes de una publicación seriada."@es,
        "L’identification de chacune des livraisons ou parties d’une publication en série."@fr ;
    rdakit:toolkitLabel "numbering of serials"@en,
        "numeración de publicaciones seriadas"@es,
        "numérotation des publications en série"@fr,
        "numrering av seriella resurser"@sv ;
    reg:hasSubproperty <http://rdaregistry.info/Elements/m/P30097>,
        <http://rdaregistry.info/Elements/m/P30098>,
        <http://rdaregistry.info/Elements/m/P30099>,
        <http://rdaregistry.info/Elements/m/P30100>,
        <http://rdaregistry.info/Elements/m/P30147>,
        <http://rdaregistry.info/Elements/m/P30148>,
        <http://rdaregistry.info/Elements/m/P30149>,
        <http://rdaregistry.info/Elements/m/P30150> ;
    reg:hasUnconstrained <http://rdaregistry.info/Elements/u/P60533> ;
    reg:lexicalAlias <http://rdaregistry.info/Elements/m/numberingOfSerials.en> ;
    reg:name "numberingOfSerials"@en ;
    reg:status <http://metadataregistry.org/uri/RegStatus/1001> ;
    rdfs:domain <http://rdaregistry.info/Elements/c/C10007> ;
    rdfs:isDefinedBy <http://rdaregistry.info/Elements/m/> ;
    skos:definition "Relates a manifestation to a designation for each of the issues or parts of a serial."@en,
        "Met une manifestation en relation avec l’identification de chacune des livraisons ou parties d’une publication en série."@fr ;
    skos:scopeNote "Numbering includes a numeral, a letter, any other character, or the combination of these with or without an accompanying caption and/or a chronological designation."@en,
        "La numérotation des publications en série peut comprendre un chiffre, une lettre, tout autre caractère ou la combinaison de ces éléments, accompagnés ou non d’une appellation (volume, numéro, etc.) et/ou d’une indication chronologique"@fr .

<http://rdaregistry.info/Elements/m/P30264> a rdf:Property ;
    rdfs:label "has related entity (manifestation)"@en ;
    reg:hasSubproperty <http://rdaregistry.info/Elements/m/P30048>,
        <http://rdaregistry.info/Elements/m/P30140>,
        <http://rdaregistry.info/Elements/m/P30265>,
        <http://rdaregistry.info/Elements/m/P30266>,
        <http://rdaregistry.info/Elements/m/P30267>,
        <http://rdaregistry.info/Elements/m/P30272>,
        <http://rdaregistry.info/Elements/m/P30273>,
        <http://rdaregistry.info/Elements/m/P30274>,
        <http://rdaregistry.info/Elements/m/datatype/P30264>,
        <http://rdaregistry.info/Elements/m/object/P30264> ;
    reg:lexicalAlias <http://rdaregistry.info/Elements/m/relatedEntityManifestation.en> ;
    reg:name "relatedEntityManifestation"@en ;
    reg:status <http://metadataregistry.org/uri/RegStatus/1001> ;
    rdfs:domain <http://rdaregistry.info/Elements/c/C10007> ;
    rdfs:isDefinedBy <http://rdaregistry.info/Elements/m/> ;
    rdfs:subPropertyOf <http://rdaregistry.info/Elements/x/P00001> ;
    skos:definition "Relates a manifestation to an entity associated with a manifestation being described."@en .

<http://rdaregistry.info/Elements/m/P30267> a rdf:Property ;
    rdfs:label "has related agent (manifestation)"@en ;
    reg:hasSubproperty <http://rdaregistry.info/Elements/m/P30268>,
        <http://rdaregistry.info/Elements/m/P30271>,
        <http://rdaregistry.info/Elements/m/datatype/P30267>,
        <http://rdaregistry.info/Elements/m/object/P30267> ;
    reg:lexicalAlias <http://rdaregistry.info/Elements/m/relatedAgentManifestation.en> ;
    reg:name "relatedAgentManifestation"@en ;
    reg:status <http://metadataregistry.org/uri/RegStatus/1001> ;
    rdfs:domain <http://rdaregistry.info/Elements/c/C10007> ;
    rdfs:isDefinedBy <http://rdaregistry.info/Elements/m/> ;
    rdfs:subPropertyOf <http://rdaregistry.info/Elements/m/P30264> ;
    skos:definition "Relates a manifestation to an agent associated with a manifestation being described."@en .

<http://rdaregistry.info/Elements/m/P30082> a rdf:Property ;
    rdfs:label "has manufacturer"@en,
        "a pour fabricant"@fr,
        "har tillverkare"@sv ;
    rdakit:instructionNumber "21.5" ;
    rdakit:toolkitDefinition "An agent responsible for printing, duplicating, casting, etc., a manifestation in a published form."@en,
        "Una persona, familia o entidad corporativa responsable de la impresión, duplicación, prensado, etc., de un recurso publicado."@es,
        "Personne, famille ou collectivité responsable de l’impression, de la reproduction, du moulage, etc. d’une ressource sous une forme publiée."@fr ;
    rdakit:toolkitLabel "manufacturer"@en,
        "fabricante"@es,
        "fabricant"@fr,
        "tillverkare"@sv ;
    reg:hasSubproperty <http://rdaregistry.info/Elements/m/P30069>,
        <http://rdaregistry.info/Elements/m/P30070>,
        <http://rdaregistry.info/Elements/m/P30071>,
        <http://rdaregistry.info/Elements/m/P30072>,
        <http://rdaregistry.info/Elements/m/P30073>,
        <http://rdaregistry.info/Elements/m/P30074>,
        <http://rdaregistry.info/Elements/m/P30075>,
        <http://rdaregistry.info/Elements/m/P30076>,
        <http://rdaregistry.info/Elements/m/P30077>,
        <http://rdaregistry.info/Elements/m/P30078>,
        <http://rdaregistry.info/Elements/m/P30215>,
        <http://rdaregistry.info/Elements/m/object/P30082> ;
    reg:hasUnconstrained <http://rdaregistry.info/Elements/u/P60443> ;
    reg:lexicalAlias <http://rdaregistry.info/Elements/m/manufacturer.en> ;
    reg:name "manufacturer"@en ;
    reg:status <http://metadataregistry.org/uri/RegStatus/1001> ;
    rdfs:domain <http://rdaregistry.info/Elements/c/C10007> ;
    rdfs:isDefinedBy <http://rdaregistry.info/Elements/m/> ;
    rdfs:subPropertyOf <http://rdaregistry.info/Elements/m/P30267> ;
    skos:definition "Relates a manifestation to an agent responsible for printing, duplicating, casting, etc., a manifestation in a published form."@en,
        "Met une manifestation en relation avec une personne, famille ou collectivité responsable de l’impression, de la reproduction, du moulage, etc. d’une ressource sous une forme publiée."@fr .

<http://rdaregistry.info/Elements/m/P30137> a rdf:Property ;
    rdfs:label "has note on manifestation"@en,
        "a pour note relative à la manifestation"@fr,
        "har anmärkning om manifestationen"@sv ;
    rdakit:instructionNumber "2.17" ;
    rdakit:toolkitDefinition "A note providing additional information about manifestation attributes."@en,
        "Una nota que proporciona información sobre los atributos de la manifestación."@es,
        "Annotation fournissant un complément d’information relatif à des attributs de la manifestation."@fr ;
    rdakit:toolkitLabel "note on manifestation"@en,
        "nota sobre la manifestación"@es,
        "note relative à la manifestation"@fr,
        "anmärkning om manifestationen"@sv ;
    reg:hasSubproperty <http://rdaregistry.info/Elements/m/P30050>,
        <http://rdaregistry.info/Elements/m/P30051>,
        <http://rdaregistry.info/Elements/m/P30052>,
        <http://rdaregistry.info/Elements/m/P30053>,
        <http://rdaregistry.info/Elements/m/P30054>,
        <http://rdaregistry.info/Elements/m/P30055>,
        <http://rdaregistry.info/Elements/m/P30056>,
        <http://rdaregistry.info/Elements/m/P30057>,
        <http://rdaregistry.info/Elements/m/P30058>,
        <http://rdaregistry.info/Elements/m/P30059>,
        <http://rdaregistry.info/Elements/m/P30062>,
        <http://rdaregistry.info/Elements/m/P30063>,
        <http://rdaregistry.info/Elements/m/P30064>,
        <http://rdaregistry.info/Elements/m/P30260> ;
    reg:hasUnconstrained <http://rdaregistry.info/Elements/u/P60470> ;
    reg:lexicalAlias <http://rdaregistry.info/Elements/m/noteOnManifestation.en> ;
    reg:name "noteOnManifestation"@en ;
    reg:status <http://metadataregistry.org/uri/RegStatus/1001> ;
    rdfs:domain <http://rdaregistry.info/Elements/c/C10007> ;
    rdfs:isDefinedBy <http://rdaregistry.info/Elements/m/> ;
    skos:definition "Relates a manifestation to a note providing additional information about manifestation attributes."@en,
        "Met une manifestation en relation avec une annotation fournissant un complément d’information relatif à des attributs de la manifestation."@fr .

<http://metadataregistry.org/uri/RegStatus/1008> a skos:Concept ;
    skos:prefLabel "Deprecated"@en .

<http://metadataregistry.org/uri/RegStatus/1001> a skos:Concept ;
    skos:prefLabel "Published"@en .

<http://rdaregistry.info/Elements/m/> dc:title "RDA Manifestation properties"@en ;
    skos:note "Properties derived from RDA elements and relationship designators with the domain of RDA Manifestation."@en ;
    foaf:homepage <http://www.rdaregistry.info/Elements/m/> .

