@prefix dc: <http://purl.org/dc/elements/1.1/> .
@prefix foaf: <http://xmlns.com/foaf/0.1/> .
@prefix rdakit: <http://metadataregistry.org/uri/profile/rdakit/> .
@prefix rdf: <http://www.w3.org/1999/02/22-rdf-syntax-ns#> .
@prefix rdfs: <http://www.w3.org/2000/01/rdf-schema#> .
@prefix reg: <http://metadataregistry.org/uri/profile/regap/> .
@prefix skos: <http://www.w3.org/2004/02/skos/core#> .
@prefix xml: <http://www.w3.org/XML/1998/namespace> .
@prefix xsd: <http://www.w3.org/2001/XMLSchema#> .

<http://rdaregistry.info/Elements/p/P70002> a rdf:Property ;
    rdfs:label "has preferred name for place"@en ;
    rdakit:instructionNumber "16.2.2" ;
    rdakit:toolkitDefinition "A name or form of name chosen to identify a place."@en ;
    rdakit:toolkitLabel "preferred name for place"@en ;
    reg:hasSubproperty <http://rdaregistry.info/Elements/p/datatype/P70002> ;
    reg:hasUnconstrained <http://rdaregistry.info/Elements/u/P60548> ;
    reg:lexicalAlias <http://rdaregistry.info/Elements/p/preferredNameForPlace.en> ;
    reg:name "preferredNameForPlace"@en ;
    reg:status <http://metadataregistry.org/uri/RegStatus/1001> ;
    rdfs:domain <http://rdaregistry.info/Elements/c/C10009> ;
    rdfs:isDefinedBy <http://rdaregistry.info/Elements/p/> ;
    rdfs:subPropertyOf <http://rdaregistry.info/Elements/p/P70001> ;
    skos:definition "Relates a place to a name or form of name chosen to identify a place."@en .

<http://rdaregistry.info/Elements/p/P70003> a rdf:Property ;
    rdfs:label "has variant name for place"@en ;
    rdakit:instructionNumber "16.2.3" ;
    rdakit:toolkitDefinition "A name or form of name by which a place is known that differs from a name or form of name chosen as a preferred name."@en ;
    rdakit:toolkitLabel "variant name for place"@en ;
    reg:hasSubproperty <http://rdaregistry.info/Elements/p/datatype/P70003> ;
    reg:hasUnconstrained <http://rdaregistry.info/Elements/u/P60880> ;
    reg:lexicalAlias <http://rdaregistry.info/Elements/p/variantNameForPlace.en> ;
    reg:name "variantNameForPlace"@en ;
    reg:status <http://metadataregistry.org/uri/RegStatus/1001> ;
    rdfs:domain <http://rdaregistry.info/Elements/c/C10009> ;
    rdfs:isDefinedBy <http://rdaregistry.info/Elements/p/> ;
    rdfs:subPropertyOf <http://rdaregistry.info/Elements/p/P70001> ;
    skos:definition "Relates a place to a name or form of name by which a place is known that differs from a name or form of name chosen as a preferred name."@en ;
    skos:scopeNote "Variant name for place includes a name or form of name found in reference sources, or a name resulting from a different transliteration of a name, etc."@en .

<http://rdaregistry.info/Elements/p/P70017> a rdf:Property ;
    rdfs:label "is subject of (place)"@en ;
    reg:hasSubproperty <http://rdaregistry.info/Elements/p/datatype/P70017>,
        <http://rdaregistry.info/Elements/p/object/P70017> ;
    reg:lexicalAlias <http://rdaregistry.info/Elements/p/subjectOfPlace.en> ;
    reg:name "subjectOfPlace"@en ;
    reg:status <http://metadataregistry.org/uri/RegStatus/1001> ;
    rdfs:domain <http://rdaregistry.info/Elements/c/C10009> ;
    rdfs:isDefinedBy <http://rdaregistry.info/Elements/p/> ;
    rdfs:subPropertyOf <http://rdaregistry.info/Elements/w/P10283> ;
    skos:definition "Relates a place to a work that is about a place."@en .

<http://rdaregistry.info/Elements/p/P70004> a rdf:Property ;
    rdfs:label "has related work (place)"@en ;
    reg:hasSubproperty <http://rdaregistry.info/Elements/p/datatype/P70004>,
        <http://rdaregistry.info/Elements/p/object/P70004> ;
    reg:lexicalAlias <http://rdaregistry.info/Elements/p/relatedWorkPlace.en> ;
    reg:name "relatedWorkPlace"@en ;
    reg:status <http://metadataregistry.org/uri/RegStatus/1001> ;
    rdfs:domain <http://rdaregistry.info/Elements/c/C10009> ;
    rdfs:isDefinedBy <http://rdaregistry.info/Elements/p/> ;
    rdfs:subPropertyOf <http://rdaregistry.info/Elements/p/P70013> ;
    skos:definition "Relates a place to a work associated with a place being described."@en .

<http://rdaregistry.info/Elements/p/P70005> a rdf:Property ;
    rdfs:label "has related expression (place)"@en ;
    reg:hasSubproperty <http://rdaregistry.info/Elements/p/datatype/P70005> ;
    reg:lexicalAlias <http://rdaregistry.info/Elements/p/relatedExpressionPlace.en> ;
    reg:name "relatedExpressionPlace"@en ;
    reg:status <http://metadataregistry.org/uri/RegStatus/1001> ;
    rdfs:domain <http://rdaregistry.info/Elements/c/C10009> ;
    rdfs:isDefinedBy <http://rdaregistry.info/Elements/p/> ;
    rdfs:subPropertyOf <http://rdaregistry.info/Elements/p/P70013> ;
    skos:definition "Relates a place to an expression associated with a place being described."@en .

<http://rdaregistry.info/Elements/p/P70006> a rdf:Property ;
    rdfs:label "has related manifestation (place)"@en ;
    reg:hasSubproperty <http://rdaregistry.info/Elements/p/datatype/P70006> ;
    reg:lexicalAlias <http://rdaregistry.info/Elements/p/relatedManifestationPlace.en> ;
    reg:name "relatedManifestationPlace"@en ;
    reg:status <http://metadataregistry.org/uri/RegStatus/1001> ;
    rdfs:domain <http://rdaregistry.info/Elements/c/C10009> ;
    rdfs:isDefinedBy <http://rdaregistry.info/Elements/p/> ;
    rdfs:subPropertyOf <http://rdaregistry.info/Elements/p/P70013> ;
    skos:definition "Relates a place to a manifestation associated with a place being described."@en .

<http://rdaregistry.info/Elements/p/P70007> a rdf:Property ;
    rdfs:label "has related item (place)"@en ;
    reg:hasSubproperty <http://rdaregistry.info/Elements/p/datatype/P70007> ;
    reg:lexicalAlias <http://rdaregistry.info/Elements/p/relatedItemPlace.en> ;
    reg:name "relatedItemPlace"@en ;
    reg:status <http://metadataregistry.org/uri/RegStatus/1001> ;
    rdfs:domain <http://rdaregistry.info/Elements/c/C10009> ;
    rdfs:isDefinedBy <http://rdaregistry.info/Elements/p/> ;
    rdfs:subPropertyOf <http://rdaregistry.info/Elements/p/P70013> ;
    skos:definition "Relates a place to an item associated with a place being described."@en .

<http://rdaregistry.info/Elements/p/P70010> a rdf:Property ;
    rdfs:label "has related place (place)"@en ;
    reg:hasSubproperty <http://rdaregistry.info/Elements/p/datatype/P70010> ;
    reg:lexicalAlias <http://rdaregistry.info/Elements/p/relatedPlacePlace.en> ;
    reg:name "relatedPlacePlace"@en ;
    reg:status <http://metadataregistry.org/uri/RegStatus/1001> ;
    rdfs:domain <http://rdaregistry.info/Elements/c/C10009> ;
    rdfs:isDefinedBy <http://rdaregistry.info/Elements/p/> ;
    rdfs:subPropertyOf <http://rdaregistry.info/Elements/p/P70013> ;
    skos:definition "Relates a place to a place associated with a place being described."@en .

<http://rdaregistry.info/Elements/p/P70011> a rdf:Property ;
    rdfs:label "has related time-span (place)"@en ;
    reg:hasSubproperty <http://rdaregistry.info/Elements/p/datatype/P70011> ;
    reg:lexicalAlias <http://rdaregistry.info/Elements/p/relatedTimespanPlace.en> ;
    reg:name "relatedTimespanPlace"@en ;
    reg:status <http://metadataregistry.org/uri/RegStatus/1001> ;
    rdfs:domain <http://rdaregistry.info/Elements/c/C10009> ;
    rdfs:isDefinedBy <http://rdaregistry.info/Elements/p/> ;
    rdfs:subPropertyOf <http://rdaregistry.info/Elements/p/P70013> ;
    skos:definition "Relates a place to a time-span associated with a place being described."@en .

<http://rdaregistry.info/Elements/p/P70012> a rdf:Property ;
    rdfs:label "has related nomen (place)"@en ;
    reg:hasSubproperty <http://rdaregistry.info/Elements/p/datatype/P70012> ;
    reg:lexicalAlias <http://rdaregistry.info/Elements/p/relatedNomenPlace.en> ;
    reg:name "relatedNomenPlace"@en ;
    reg:status <http://metadataregistry.org/uri/RegStatus/1001> ;
    rdfs:domain <http://rdaregistry.info/Elements/c/C10009> ;
    rdfs:isDefinedBy <http://rdaregistry.info/Elements/p/> ;
    rdfs:subPropertyOf <http://rdaregistry.info/Elements/p/P70013> ;
    skos:definition "Relates a place to a nomen associated with a place being described."@en .

<http://rdaregistry.info/Elements/p/P70001> a rdf:Property ;
    rdfs:label "has name of place"@en ;
    rdakit:instructionNumber "16.2" ;
    rdakit:toolkitDefinition "A word, character, or group of words or characters by which a place is known."@en ;
    rdakit:toolkitLabel "name of place"@en ;
    reg:hasSubproperty <http://rdaregistry.info/Elements/p/datatype/P70001> ;
    reg:hasUnconstrained <http://rdaregistry.info/Elements/u/P60366> ;
    reg:lexicalAlias <http://rdaregistry.info/Elements/p/nameOfPlace.en> ;
    reg:name "nameOfPlace"@en ;
    reg:status <http://metadataregistry.org/uri/RegStatus/1001> ;
    rdfs:domain <http://rdaregistry.info/Elements/c/C10009> ;
    rdfs:isDefinedBy <http://rdaregistry.info/Elements/p/> ;
    skos:definition "Relates a place to a word, character, or group of words and/or characters by which a place is known."@en .

<http://rdaregistry.info/Elements/p/P70014> a rdf:Property ;
    rdfs:label "has related person (place)"@en ;
    reg:hasSubproperty <http://rdaregistry.info/Elements/p/P70014>,
        <http://rdaregistry.info/Elements/p/datatype/P70014> ;
    reg:lexicalAlias <http://rdaregistry.info/Elements/p/relatedPersonPlace.en> ;
    reg:name "relatedPersonPlace"@en ;
    reg:status <http://metadataregistry.org/uri/RegStatus/1001> ;
    rdfs:domain <http://rdaregistry.info/Elements/c/C10009> ;
    rdfs:isDefinedBy <http://rdaregistry.info/Elements/p/> ;
    rdfs:subPropertyOf <http://rdaregistry.info/Elements/p/P70008> ;
    skos:definition "Relates a place to a person associated with a place being described."@en .

<http://rdaregistry.info/Elements/p/P70015> a rdf:Property ;
    rdfs:label "has related family (place)"@en ;
    reg:hasSubproperty <http://rdaregistry.info/Elements/p/P70015>,
        <http://rdaregistry.info/Elements/p/datatype/P70015> ;
    reg:lexicalAlias <http://rdaregistry.info/Elements/p/relatedFamilyPlace.en> ;
    reg:name "relatedFamilyPlace"@en ;
    reg:status <http://metadataregistry.org/uri/RegStatus/1001> ;
    rdfs:domain <http://rdaregistry.info/Elements/c/C10009> ;
    rdfs:isDefinedBy <http://rdaregistry.info/Elements/p/> ;
    rdfs:subPropertyOf <http://rdaregistry.info/Elements/p/P70009> ;
    skos:definition "Relates a place to a family associated with a place being described."@en .

<http://rdaregistry.info/Elements/p/P70016> a rdf:Property ;
    rdfs:label "has related corporate body (place)"@en ;
    reg:hasSubproperty <http://rdaregistry.info/Elements/p/P70016>,
        <http://rdaregistry.info/Elements/p/datatype/P70016> ;
    reg:lexicalAlias <http://rdaregistry.info/Elements/p/relatedCorporateBodyPlace.en> ;
    reg:name "relatedCorporateBodyPlace"@en ;
    reg:status <http://metadataregistry.org/uri/RegStatus/1001> ;
    rdfs:domain <http://rdaregistry.info/Elements/c/C10009> ;
    rdfs:isDefinedBy <http://rdaregistry.info/Elements/p/> ;
    rdfs:subPropertyOf <http://rdaregistry.info/Elements/p/P70009> ;
    skos:definition "Relates a place to a corporate body associated with a place being described."@en .

<http://rdaregistry.info/Elements/p/P70008> a rdf:Property ;
    rdfs:label "has related agent (place)"@en ;
    reg:hasSubproperty <http://rdaregistry.info/Elements/p/P70009>,
        <http://rdaregistry.info/Elements/p/P70014>,
        <http://rdaregistry.info/Elements/p/datatype/P70008> ;
    reg:lexicalAlias <http://rdaregistry.info/Elements/p/relatedAgentPlace.en> ;
    reg:name "relatedAgentPlace"@en ;
    reg:status <http://metadataregistry.org/uri/RegStatus/1001> ;
    rdfs:domain <http://rdaregistry.info/Elements/c/C10009> ;
    rdfs:isDefinedBy <http://rdaregistry.info/Elements/p/> ;
    rdfs:subPropertyOf <http://rdaregistry.info/Elements/p/P70013> ;
    skos:definition "Relates a place to an agent associated with a place being described."@en .

<http://rdaregistry.info/Elements/p/P70009> a rdf:Property ;
    rdfs:label "has related collective agent (place)"@en ;
    reg:hasSubproperty <http://rdaregistry.info/Elements/p/P70015>,
        <http://rdaregistry.info/Elements/p/P70016>,
        <http://rdaregistry.info/Elements/p/datatype/P70009> ;
    reg:lexicalAlias <http://rdaregistry.info/Elements/p/relatedCollectiveAgentPlace.en> ;
    reg:name "relatedCollectiveAgentPlace"@en ;
    reg:status <http://metadataregistry.org/uri/RegStatus/1001> ;
    rdfs:domain <http://rdaregistry.info/Elements/c/C10009> ;
    rdfs:isDefinedBy <http://rdaregistry.info/Elements/p/> ;
    rdfs:subPropertyOf <http://rdaregistry.info/Elements/p/P70008> ;
    skos:definition "Relates a place to a collective agent associated with a place being described."@en .

<http://rdaregistry.info/Elements/p/P70013> a rdf:Property ;
    rdfs:label "has related entity (place)"@en ;
    reg:hasSubproperty <http://rdaregistry.info/Elements/p/P70004>,
        <http://rdaregistry.info/Elements/p/P70005>,
        <http://rdaregistry.info/Elements/p/P70006>,
        <http://rdaregistry.info/Elements/p/P70007>,
        <http://rdaregistry.info/Elements/p/P70008>,
        <http://rdaregistry.info/Elements/p/P70010>,
        <http://rdaregistry.info/Elements/p/P70011>,
        <http://rdaregistry.info/Elements/p/P70012>,
        <http://rdaregistry.info/Elements/p/datatype/P70013> ;
    reg:lexicalAlias <http://rdaregistry.info/Elements/p/relatedEntityPlace.en> ;
    reg:name "relatedEntityPlace"@en ;
    reg:status <http://metadataregistry.org/uri/RegStatus/1001> ;
    rdfs:domain <http://rdaregistry.info/Elements/c/C10009> ;
    rdfs:isDefinedBy <http://rdaregistry.info/Elements/p/> ;
    rdfs:subPropertyOf <http://rdaregistry.info/Elements/x/P00001> ;
    skos:definition "Relates a place to an entity associated with a place being described."@en .

<http://metadataregistry.org/uri/RegStatus/1001> a skos:Concept ;
    skos:prefLabel "Published"@en .

<http://rdaregistry.info/Elements/p/> dc:title "RDA Place properties"@en ;
    skos:note "Properties derived from RDA elements and relationship designators with the domain of RDA Place."@en .

