@prefix dc: <http://purl.org/dc/elements/1.1/> .
@prefix foaf: <http://xmlns.com/foaf/0.1/> .
@prefix rdf: <http://www.w3.org/1999/02/22-rdf-syntax-ns#> .
@prefix rdfs: <http://www.w3.org/2000/01/rdf-schema#> .
@prefix reg: <http://metadataregistry.org/uri/profile/regap/> .
@prefix skos: <http://www.w3.org/2004/02/skos/core#> .
@prefix xml: <http://www.w3.org/XML/1998/namespace> .
@prefix xsd: <http://www.w3.org/2001/XMLSchema#> .

<http://rdaregistry.info/Elements/t/P70014> a rdf:Property ;
    rdfs:label "is subject of (time-span)"@en ;
    reg:hasSubproperty <http://rdaregistry.info/Elements/t/datatype/P70014>,
        <http://rdaregistry.info/Elements/t/object/P70014> ;
    reg:lexicalAlias <http://rdaregistry.info/Elements/t/subjectOfTimespan.en> ;
    reg:name "subjectOfTimespan"@en ;
    reg:status <http://metadataregistry.org/uri/RegStatus/1001> ;
    rdfs:domain <http://rdaregistry.info/Elements/c/C10010> ;
    rdfs:isDefinedBy <http://rdaregistry.info/Elements/t/> ;
    rdfs:subPropertyOf <http://rdaregistry.info/Elements/w/P10283> ;
    skos:definition "Relates a time-span to a work that is about a time-span being described."@en .

<http://rdaregistry.info/Elements/t/P70001> a rdf:Property ;
    rdfs:label "has related work (time-span)"@en ;
    reg:hasSubproperty <http://rdaregistry.info/Elements/t/datatype/P70001>,
        <http://rdaregistry.info/Elements/t/object/P70001> ;
    reg:lexicalAlias <http://rdaregistry.info/Elements/t/relatedWorkTimespan.en> ;
    reg:name "relatedWorkTimespan"@en ;
    reg:status <http://metadataregistry.org/uri/RegStatus/1001> ;
    rdfs:domain <http://rdaregistry.info/Elements/c/C10010> ;
    rdfs:isDefinedBy <http://rdaregistry.info/Elements/t/> ;
    rdfs:subPropertyOf <http://rdaregistry.info/Elements/t/P70010> ;
    skos:definition "Relates a time-span to a work associated with a time-span being described."@en .

<http://rdaregistry.info/Elements/t/P70002> a rdf:Property ;
    rdfs:label "has related expression (time-span)"@en ;
    reg:hasSubproperty <http://rdaregistry.info/Elements/t/datatype/P70002>,
        <http://rdaregistry.info/Elements/t/object/P70002> ;
    reg:lexicalAlias <http://rdaregistry.info/Elements/t/relatedExpressionTimespan.en> ;
    reg:name "relatedExpressionTimespan"@en ;
    reg:status <http://metadataregistry.org/uri/RegStatus/1001> ;
    rdfs:domain <http://rdaregistry.info/Elements/c/C10010> ;
    rdfs:isDefinedBy <http://rdaregistry.info/Elements/t/> ;
    rdfs:subPropertyOf <http://rdaregistry.info/Elements/t/P70010> ;
    skos:definition "Relates a time-span to an expression associated with a time-span being described."@en .

<http://rdaregistry.info/Elements/t/P70003> a rdf:Property ;
    rdfs:label "has related manifestation (time-span)"@en ;
    reg:hasSubproperty <http://rdaregistry.info/Elements/t/datatype/P70003>,
        <http://rdaregistry.info/Elements/t/object/P70003> ;
    reg:lexicalAlias <http://rdaregistry.info/Elements/t/relatedManifestationTimespan.en> ;
    reg:name "relatedManifestationTimespan"@en ;
    reg:status <http://metadataregistry.org/uri/RegStatus/1001> ;
    rdfs:domain <http://rdaregistry.info/Elements/c/C10010> ;
    rdfs:isDefinedBy <http://rdaregistry.info/Elements/t/> ;
    rdfs:subPropertyOf <http://rdaregistry.info/Elements/t/P70010> ;
    skos:definition "Relates a time-span to a manifestation associated with a time-span being described."@en .

<http://rdaregistry.info/Elements/t/P70004> a rdf:Property ;
    rdfs:label "has related item (time-span)"@en ;
    reg:hasSubproperty <http://rdaregistry.info/Elements/t/datatype/P70004>,
        <http://rdaregistry.info/Elements/t/object/P70004> ;
    reg:lexicalAlias <http://rdaregistry.info/Elements/t/relatedItemTimespan.en> ;
    reg:name "relatedItemTimespan"@en ;
    reg:status <http://metadataregistry.org/uri/RegStatus/1001> ;
    rdfs:domain <http://rdaregistry.info/Elements/c/C10010> ;
    rdfs:isDefinedBy <http://rdaregistry.info/Elements/t/> ;
    rdfs:subPropertyOf <http://rdaregistry.info/Elements/t/P70010> ;
    skos:definition "Relates a time-span to an item associated with a time-span being described."@en .

<http://rdaregistry.info/Elements/t/P70007> a rdf:Property ;
    rdfs:label "has related place (time-span)"@en ;
    reg:hasSubproperty <http://rdaregistry.info/Elements/t/datatype/P70007>,
        <http://rdaregistry.info/Elements/t/object/P70007> ;
    reg:lexicalAlias <http://rdaregistry.info/Elements/t/relatedPlaceTimespan.en> ;
    reg:name "relatedPlaceTimespan"@en ;
    reg:status <http://metadataregistry.org/uri/RegStatus/1001> ;
    rdfs:domain <http://rdaregistry.info/Elements/c/C10010> ;
    rdfs:isDefinedBy <http://rdaregistry.info/Elements/t/> ;
    rdfs:subPropertyOf <http://rdaregistry.info/Elements/t/P70010> ;
    skos:definition "Relates a time-span to a place associated with a time-span being described."@en .

<http://rdaregistry.info/Elements/t/P70008> a rdf:Property ;
    rdfs:label "has related time-span (time-span)"@en ;
    reg:hasSubproperty <http://rdaregistry.info/Elements/t/datatype/P70008>,
        <http://rdaregistry.info/Elements/t/object/P70008> ;
    reg:lexicalAlias <http://rdaregistry.info/Elements/t/relatedTimespanTimespan.en> ;
    reg:name "relatedTimespanTimespan"@en ;
    reg:status <http://metadataregistry.org/uri/RegStatus/1001> ;
    rdfs:domain <http://rdaregistry.info/Elements/c/C10010> ;
    rdfs:isDefinedBy <http://rdaregistry.info/Elements/t/> ;
    rdfs:subPropertyOf <http://rdaregistry.info/Elements/t/P70010> ;
    skos:definition "Relates a time-span to a time-span associated with a time-span being described."@en .

<http://rdaregistry.info/Elements/t/P70009> a rdf:Property ;
    rdfs:label "has related nomen (time-span)"@en ;
    reg:hasSubproperty <http://rdaregistry.info/Elements/t/datatype/P70009>,
        <http://rdaregistry.info/Elements/t/object/P70009> ;
    reg:lexicalAlias <http://rdaregistry.info/Elements/t/relatedNomenTimespan.en> ;
    reg:name "relatedNomenTimespan"@en ;
    reg:status <http://metadataregistry.org/uri/RegStatus/1001> ;
    rdfs:domain <http://rdaregistry.info/Elements/c/C10010> ;
    rdfs:isDefinedBy <http://rdaregistry.info/Elements/t/> ;
    rdfs:subPropertyOf <http://rdaregistry.info/Elements/t/P70010> ;
    skos:definition "Relates a time-span to a nomen associated with a time-span being described."@en .

<http://rdaregistry.info/Elements/t/P70011> a rdf:Property ;
    rdfs:label "has related person (time-span)"@en ;
    reg:hasSubproperty <http://rdaregistry.info/Elements/t/datatype/P70011>,
        <http://rdaregistry.info/Elements/t/object/P70011> ;
    reg:lexicalAlias <http://rdaregistry.info/Elements/t/relatedPersonTimespan.en> ;
    reg:name "relatedPersonTimespan"@en ;
    reg:status <http://metadataregistry.org/uri/RegStatus/1001> ;
    rdfs:domain <http://rdaregistry.info/Elements/c/C10010> ;
    rdfs:isDefinedBy <http://rdaregistry.info/Elements/t/> ;
    rdfs:subPropertyOf <http://rdaregistry.info/Elements/t/P70005> ;
    skos:definition "Relates a time-span to a person associated with a time-span being described."@en .

<http://rdaregistry.info/Elements/t/P70012> a rdf:Property ;
    rdfs:label "has related family (time-span)"@en ;
    reg:hasSubproperty <http://rdaregistry.info/Elements/t/datatype/P70012>,
        <http://rdaregistry.info/Elements/t/object/P70012> ;
    reg:lexicalAlias <http://rdaregistry.info/Elements/t/relatedFamilyTimespan.en> ;
    reg:name "relatedFamilyTimespan"@en ;
    reg:status <http://metadataregistry.org/uri/RegStatus/1001> ;
    rdfs:domain <http://rdaregistry.info/Elements/c/C10010> ;
    rdfs:isDefinedBy <http://rdaregistry.info/Elements/t/> ;
    rdfs:subPropertyOf <http://rdaregistry.info/Elements/t/P70006> ;
    skos:definition "Relates a time-span to a family associated with a time-span being described."@en .

<http://rdaregistry.info/Elements/t/P70013> a rdf:Property ;
    rdfs:label "has related corporate body (time-span)"@en ;
    reg:hasSubproperty <http://rdaregistry.info/Elements/t/datatype/P70013>,
        <http://rdaregistry.info/Elements/t/object/P70013> ;
    reg:lexicalAlias <http://rdaregistry.info/Elements/t/relatedCorporateBodyTimespan.en> ;
    reg:name "relatedCorporateBodyTimespan"@en ;
    reg:status <http://metadataregistry.org/uri/RegStatus/1001> ;
    rdfs:domain <http://rdaregistry.info/Elements/c/C10010> ;
    rdfs:isDefinedBy <http://rdaregistry.info/Elements/t/> ;
    rdfs:subPropertyOf <http://rdaregistry.info/Elements/t/P70006> ;
    skos:definition "Relates a time-span to a corporate body associated with a time-span being described."@en .

<http://rdaregistry.info/Elements/t/P70005> a rdf:Property ;
    rdfs:label "has related agent (time-span)"@en ;
    reg:hasSubproperty <http://rdaregistry.info/Elements/t/P70006>,
        <http://rdaregistry.info/Elements/t/P70011>,
        <http://rdaregistry.info/Elements/t/datatype/P70005>,
        <http://rdaregistry.info/Elements/t/object/P70005> ;
    reg:lexicalAlias <http://rdaregistry.info/Elements/t/relatedAgentTimespan.en> ;
    reg:name "relatedAgentTimespan"@en ;
    reg:status <http://metadataregistry.org/uri/RegStatus/1001> ;
    rdfs:domain <http://rdaregistry.info/Elements/c/C10010> ;
    rdfs:isDefinedBy <http://rdaregistry.info/Elements/t/> ;
    rdfs:subPropertyOf <http://rdaregistry.info/Elements/t/P70010> ;
    skos:definition "Relates a time-span to an agent associated with a time-span being described."@en .

<http://rdaregistry.info/Elements/t/P70006> a rdf:Property ;
    rdfs:label "has related collective agent (time-span)"@en ;
    reg:hasSubproperty <http://rdaregistry.info/Elements/t/P70012>,
        <http://rdaregistry.info/Elements/t/P70013>,
        <http://rdaregistry.info/Elements/t/datatype/P70006>,
        <http://rdaregistry.info/Elements/t/object/P70006> ;
    reg:lexicalAlias <http://rdaregistry.info/Elements/t/relatedCollectiveAgentTimespan.en> ;
    reg:name "relatedCollectiveAgentTimespan"@en ;
    reg:status <http://metadataregistry.org/uri/RegStatus/1001> ;
    rdfs:domain <http://rdaregistry.info/Elements/c/C10010> ;
    rdfs:isDefinedBy <http://rdaregistry.info/Elements/t/> ;
    rdfs:subPropertyOf <http://rdaregistry.info/Elements/t/P70005> ;
    skos:definition "Relates a time-span to a collective agent associated with a time-span being described."@en .

<http://rdaregistry.info/Elements/t/P70010> a rdf:Property ;
    rdfs:label "has related entity (time-span)"@en ;
    reg:hasSubproperty <http://rdaregistry.info/Elements/t/P70001>,
        <http://rdaregistry.info/Elements/t/P70002>,
        <http://rdaregistry.info/Elements/t/P70003>,
        <http://rdaregistry.info/Elements/t/P70004>,
        <http://rdaregistry.info/Elements/t/P70005>,
        <http://rdaregistry.info/Elements/t/P70007>,
        <http://rdaregistry.info/Elements/t/P70008>,
        <http://rdaregistry.info/Elements/t/P70009>,
        <http://rdaregistry.info/Elements/t/datatype/P70010>,
        <http://rdaregistry.info/Elements/t/object/P70010> ;
    reg:lexicalAlias <http://rdaregistry.info/Elements/t/relatedEntityTimespan.en> ;
    reg:name "relatedEntityTimespan"@en ;
    reg:status <http://metadataregistry.org/uri/RegStatus/1001> ;
    rdfs:domain <http://rdaregistry.info/Elements/c/C10010> ;
    rdfs:isDefinedBy <http://rdaregistry.info/Elements/t/> ;
    rdfs:subPropertyOf <http://rdaregistry.info/Elements/x/P00001> ;
    skos:definition "Relates a time-span to an entity associated with a time-span being described."@en .

<http://metadataregistry.org/uri/RegStatus/1001> a skos:Concept ;
    skos:prefLabel "Published"@en .

<http://rdaregistry.info/Elements/t/> dc:title "RDA Time-span properties"@en ;
    skos:note "Properties derived from RDA elements and relationship designators with the domain of RDA Time-span."@en .

