<?xml version="1.0"?>
<rdf:RDF xmlns="http://purl.bdrc.io/ontology/"
     xml:base="http://purl.bdrc.io/ontology/"
     xmlns:bdd="http://purl.bdrc.io/data/"
     xmlns:bf="http://id.loc.gov/ontologies/bibframe/"
     xmlns:owl="http://www.w3.org/2002/07/owl#"
     xmlns:xsd="http://www.w3.org/2001/XMLSchema#"
     xmlns:skos="http://www.w3.org/2004/02/skos/core#"
     xmlns:admin="http://purl.bdrc.io/ontology/admin/"
     xmlns:rdfs="http://www.w3.org/2000/01/rdf-schema#"
     xmlns:bdo="http://purl.bdrc.io/ontology/"
     xmlns:bdr="http://purl.bdrc.io/resource/"
     xmlns:rdf="http://www.w3.org/1999/02/22-rdf-syntax-ns#"
     xmlns:xml="http://www.w3.org/XML/1998/namespace"
     xmlns:dcterms="http://purl.org/dc/terms/"
     xmlns:foaf="http://xmlns.com/foaf/0.1/">
    <owl:Ontology rdf:about="http://purl.bdrc.io/ontology/">
        <rdfs:label rdf:datatype="http://www.w3.org/2001/XMLSchema#string">BDRC Ontology</rdfs:label>
        <owl:versionInfo rdf:datatype="http://www.w3.org/2001/XMLSchema#string">0.1</owl:versionInfo>
    </owl:Ontology>
    


    <!-- 
    ///////////////////////////////////////////////////////////////////////////////////////
    //
    // Annotation properties
    //
    ///////////////////////////////////////////////////////////////////////////////////////
     -->

    


    <!-- http://purl.bdrc.io/ontology/dataTypeExpression -->

    <owl:AnnotationProperty rdf:about="http://purl.bdrc.io/ontology/dataTypeExpression"/>
    


    <!-- http://purl.bdrc.io/ontology/external -->

    <owl:AnnotationProperty rdf:about="http://purl.bdrc.io/ontology/external">
        <rdfs:range rdf:resource="http://purl.bdrc.io/ontology/common#External"/>
    </owl:AnnotationProperty>
    


    <!-- http://purl.bdrc.io/ontology/inferSubTree -->

    <owl:AnnotationProperty rdf:about="http://purl.bdrc.io/ontology/inferSubTree">
        <rdfs:range rdf:resource="http://www.w3.org/2001/XMLSchema#boolean"/>
    </owl:AnnotationProperty>
    


    <!-- http://purl.bdrc.io/ontology/migration_exception -->

    <owl:AnnotationProperty rdf:about="http://purl.bdrc.io/ontology/migration_exception">
        <rdfs:range rdf:resource="http://www.w3.org/2001/XMLSchema#string"/>
    </owl:AnnotationProperty>
    


    <!-- http://purl.bdrc.io/ontology/note -->

    <owl:AnnotationProperty rdf:about="http://purl.bdrc.io/ontology/note">
        <rdfs:comment>the :note annotation adds langauge tagged string and optionally a reference to a Work and a simpe text description of a location in a Work, e.g., &quot;pp. 231-3&quot;.

In the XML db the notes are restricted to a limited set of items such as top-level resources and Outline Nodes, Place Events and so on. In this model there are no limitations on where notes can be attached. They can be attached directly to any owl:NamedIndividual or property. In particular one could add a note to the per:name property on an individual that provides evidence for the particular per:name assertion.</rdfs:comment>
        <rdfs:range rdf:resource="http://purl.bdrc.io/ontology/Note"/>
    </owl:AnnotationProperty>
    


    <!-- http://purl.bdrc.io/ontology/noteLocationStatement -->

    <owl:AnnotationProperty rdf:about="http://purl.bdrc.io/ontology/noteLocationStatement">
        <rdfs:comment xml:lang="en">A location statement for where in the :noteWork to look for the :noteText</rdfs:comment>
        <rdfs:comment xml:lang="en">Migration hint: the @location of the &lt;x:note/&gt;.</rdfs:comment>
        <rdfs:label xml:lang="en">location</rdfs:label>
        <rdfs:range rdf:resource="http://www.w3.org/2001/XMLSchema#string"/>
        <rdfs:domain rdf:resource="http://purl.bdrc.io/ontology/Note"/>
    </owl:AnnotationProperty>
    


    <!-- http://purl.bdrc.io/ontology/noteText -->

    <owl:AnnotationProperty rdf:about="http://purl.bdrc.io/ontology/noteText">
        <rdfs:range rdf:resource="http://www.w3.org/1999/02/22-rdf-syntax-ns#PlainLiteral"/>
        <rdfs:domain rdf:resource="http://purl.bdrc.io/ontology/Note"/>
    </owl:AnnotationProperty>
    


    <!-- http://purl.bdrc.io/ontology/noteWork -->

    <owl:AnnotationProperty rdf:about="http://purl.bdrc.io/ontology/noteWork">
        <rdfs:comment xml:lang="en">The source Work for the noteContent</rdfs:comment>
        <rdfs:label xml:lang="en">work</rdfs:label>
        <rdfs:range rdf:resource="http://purl.bdrc.io/ontology/Work"/>
        <rdfs:domain rdf:resource="http://purl.bdrc.io/ontology/Note"/>
    </owl:AnnotationProperty>
    


    <!-- http://purl.bdrc.io/ontology/seeAlso -->

    <owl:AnnotationProperty rdf:about="http://purl.bdrc.io/ontology/seeAlso">
        <rdfs:range rdf:resource="http://purl.bdrc.io/ontology/Topic"/>
        <rdfs:domain rdf:resource="http://purl.bdrc.io/ontology/Topic"/>
    </owl:AnnotationProperty>
    


    <!-- http://purl.bdrc.io/ontology/status -->

    <owl:AnnotationProperty rdf:about="http://purl.bdrc.io/ontology/status">
        <rdfs:range rdf:resource="http://purl.bdrc.io/ontology/StatusType"/>
        <rdfs:domain rdf:resource="http://purl.bdrc.io/ontology/Entity"/>
    </owl:AnnotationProperty>
    


    <!-- http://purl.bdrc.io/ontology/taxElementOfRelation -->

    <owl:AnnotationProperty rdf:about="http://purl.bdrc.io/ontology/taxElementOfRelation">
        <rdfs:comment xml:lang="en">Identifies a relation to be used as the element of relation for a custom taxonomy</rdfs:comment>
        <rdfs:label xml:lang="en">taxonomy element of relation</rdfs:label>
        <rdfs:range rdf:resource="http://www.w3.org/2002/07/owl#ObjectProperty"/>
        <rdfs:domain rdf:resource="http://purl.bdrc.io/ontology/Taxonomy"/>
    </owl:AnnotationProperty>
    


    <!-- http://purl.bdrc.io/ontology/taxSubclassRelation -->

    <owl:AnnotationProperty rdf:about="http://purl.bdrc.io/ontology/taxSubclassRelation">
        <rdfs:comment xml:lang="en">This identifies a property that is used in a custom taxonomy to represent the subclass relation for the taxonomy</rdfs:comment>
        <rdfs:label xml:lang="en">taxonomy subclass relation</rdfs:label>
        <rdfs:range rdf:resource="http://www.w3.org/2002/07/owl#ObjectProperty"/>
        <rdfs:domain rdf:resource="http://purl.bdrc.io/ontology/Taxonomy"/>
    </owl:AnnotationProperty>
    


    <!-- http://purl.bdrc.io/ontology/admin/conversionAnnotations -->

    <owl:AnnotationProperty rdf:about="http://purl.bdrc.io/ontology/admin/conversionAnnotations"/>
    


    <!-- http://purl.bdrc.io/ontology/admin/convertProperty -->

    <owl:AnnotationProperty rdf:about="http://purl.bdrc.io/ontology/admin/convertProperty">
        <rdfs:comment xml:lang="en">this annotation indicates that the annotated property is to be converted to some other expression, typically to a form that is expressed in terms of a common 3rd-party ontology such as bibframe or foaf.

The value of this property should be an explanation of the needed conversion as an rdf:langString</rdfs:comment>
        <rdfs:subPropertyOf rdf:resource="http://purl.bdrc.io/ontology/admin/conversionAnnotations"/>
        <rdfs:range rdf:resource="http://www.w3.org/1999/02/22-rdf-syntax-ns#PlainLiteral"/>
    </owl:AnnotationProperty>
    


    <!-- http://purl.bdrc.io/ontology/admin/convertToClass -->

    <owl:AnnotationProperty rdf:about="http://purl.bdrc.io/ontology/admin/convertToClass">
        <rdfs:comment xml:lang="en">this annotation is used to indicate that uses of the annotated class are to be replaced by the inidcated class</rdfs:comment>
        <rdfs:label xml:lang="en">convert to Class</rdfs:label>
        <rdfs:subPropertyOf rdf:resource="http://purl.bdrc.io/ontology/admin/conversionAnnotations"/>
        <rdfs:range rdf:resource="http://www.w3.org/2002/07/owl#Thing"/>
        <rdfs:domain rdf:resource="http://www.w3.org/2002/07/owl#Thing"/>
    </owl:AnnotationProperty>
    


    <!-- http://purl.bdrc.io/ontology/admin/convertToProperty -->

    <owl:AnnotationProperty rdf:about="http://purl.bdrc.io/ontology/admin/convertToProperty">
        <rdfs:comment xml:lang="en">Indicates that the annotated property is to be converted directly to a statement in terms of another property. The value of this annotation is the target property to convert to.</rdfs:comment>
        <rdfs:subPropertyOf rdf:resource="http://purl.bdrc.io/ontology/admin/conversionAnnotations"/>
    </owl:AnnotationProperty>
    


    <!-- http://purl.bdrc.io/ontology/admin/convertValueToClass -->

    <owl:AnnotationProperty rdf:about="http://purl.bdrc.io/ontology/admin/convertValueToClass">
        <rdfs:comment xml:lang="en">Indicates that the value of the property being converted is to be an instance of the designated class</rdfs:comment>
        <rdfs:subPropertyOf rdf:resource="http://purl.bdrc.io/ontology/admin/conversionAnnotations"/>
    </owl:AnnotationProperty>
    


    <!-- http://purl.bdrc.io/ontology/admin/logDate -->

    <owl:AnnotationProperty rdf:about="http://purl.bdrc.io/ontology/admin/logDate">
        <rdfs:comment xml:lang="en">When the update was performed</rdfs:comment>
        <rdfs:label xml:lang="en">date</rdfs:label>
        <rdfs:range rdf:resource="http://www.w3.org/2001/XMLSchema#dateTime"/>
        <rdfs:domain rdf:resource="http://purl.bdrc.io/ontology/admin/LogEntry"/>
    </owl:AnnotationProperty>
    


    <!-- http://purl.bdrc.io/ontology/admin/logEntry -->

    <owl:AnnotationProperty rdf:about="http://purl.bdrc.io/ontology/admin/logEntry">
        <rdfs:comment xml:lang="en">Log entry for updates to BDRC resources</rdfs:comment>
        <rdfs:label xml:lang="en">log entry</rdfs:label>
        <rdfs:range rdf:resource="http://purl.bdrc.io/ontology/admin/LogEntry"/>
        <rdfs:domain rdf:resource="http://purl.bdrc.io/ontology/Entity"/>
    </owl:AnnotationProperty>
    


    <!-- http://purl.bdrc.io/ontology/admin/logMessage -->

    <owl:AnnotationProperty rdf:about="http://purl.bdrc.io/ontology/admin/logMessage">
        <rdfs:comment xml:lang="en">Explanation of the update</rdfs:comment>
        <rdfs:label xml:lang="en">message</rdfs:label>
        <rdfs:range rdf:resource="http://www.w3.org/1999/02/22-rdf-syntax-ns#PlainLiteral"/>
        <rdfs:domain rdf:resource="http://purl.bdrc.io/ontology/admin/LogEntry"/>
    </owl:AnnotationProperty>
    


    <!-- http://purl.bdrc.io/ontology/admin/logWho -->

    <owl:AnnotationProperty rdf:about="http://purl.bdrc.io/ontology/admin/logWho">
        <rdfs:comment xml:lang="en">who performed the updated being logged</rdfs:comment>
        <rdfs:label xml:lang="en">who</rdfs:label>
        <rdfs:range rdf:resource="http://xmlns.com/foaf/0.1/Agent"/>
        <rdfs:domain rdf:resource="http://purl.bdrc.io/ontology/admin/LogEntry"/>
    </owl:AnnotationProperty>
    


    <!-- http://purl.bdrc.io/ontology/admin/place_TLM_accession -->

    <owl:AnnotationProperty rdf:about="http://purl.bdrc.io/ontology/admin/place_TLM_accession">
        <rdfs:comment>The accession attribute records the next accession number to be allocated for the Library. The num should be a 6 digit zero filled string initialized to &quot;000001&quot;. This number is incremented each time a new holdng is added for this library.</rdfs:comment>
        <rdfs:label xml:lang="en">accession</rdfs:label>
        <rdfs:range rdf:resource="http://www.w3.org/2001/XMLSchema#string"/>
        <rdfs:domain rdf:resource="http://purl.bdrc.io/ontology/Place"/>
    </owl:AnnotationProperty>
    


    <!-- http://purl.bdrc.io/ontology/admin/place_TLM_admin -->

    <owl:AnnotationProperty rdf:about="http://purl.bdrc.io/ontology/admin/place_TLM_admin">
        <rdfs:comment>The admin property records the name of the group of users that are permitted to update the Library and Monastery profiles for the Library. The group name will conventionally be named by lower-casing the hasTLM_code property value and appending &quot;Admin&quot;. For example, &quot;dzlAdmin&quot;</rdfs:comment>
        <rdfs:label xml:lang="en">tlm admin group</rdfs:label>
        <rdfs:range rdf:resource="http://www.w3.org/2001/XMLSchema#string"/>
        <rdfs:domain rdf:resource="http://purl.bdrc.io/ontology/Place"/>
    </owl:AnnotationProperty>
    


    <!-- http://purl.bdrc.io/ontology/admin/place_TLM_adminEmail -->

    <owl:AnnotationProperty rdf:about="http://purl.bdrc.io/ontology/admin/place_TLM_adminEmail">
        <rdfs:comment>The admin email is used to send requests for new users to be added to the Library.</rdfs:comment>
        <rdfs:label xml:lang="en">tlm admin email</rdfs:label>
        <rdfs:range rdf:resource="http://www.w3.org/2001/XMLSchema#string"/>
        <rdfs:domain rdf:resource="http://purl.bdrc.io/ontology/Place"/>
    </owl:AnnotationProperty>
    


    <!-- http://purl.bdrc.io/ontology/admin/place_TLM_code -->

    <owl:AnnotationProperty rdf:about="http://purl.bdrc.io/ontology/admin/place_TLM_code">
        <rdfs:comment>the code attribute records a unique 3-latin-letter code for the Library. For example, DZL would be reasonable for Dzongsar Library. The code along with the num attribute are used to create RIDs for Works that are added by the library. RIDs will take the form of: W1TLMDZL000001</rdfs:comment>
        <rdfs:label xml:lang="en">tlm code</rdfs:label>
        <rdfs:range rdf:resource="http://www.w3.org/2001/XMLSchema#string"/>
        <rdfs:domain rdf:resource="http://purl.bdrc.io/ontology/Place"/>
    </owl:AnnotationProperty>
    


    <!-- http://purl.bdrc.io/ontology/admin/place_TLM_librarian -->

    <owl:AnnotationProperty rdf:about="http://purl.bdrc.io/ontology/admin/place_TLM_librarian">
        <rdfs:comment xml:lang="en">The librarian property records the name of the group of users that are permitted to add/update/delete Library holdings. The group name will conventionally be named by lower-casing the TLM/code and appending &quot;librarian&quot;. for example, &quot;dzllibrarian&quot;</rdfs:comment>
        <rdfs:label xml:lang="en">tlm librarian group</rdfs:label>
        <rdfs:range rdf:resource="http://www.w3.org/2001/XMLSchema#string"/>
        <rdfs:domain rdf:resource="http://purl.bdrc.io/ontology/Place"/>
    </owl:AnnotationProperty>
    


    <!-- http://purl.bdrc.io/ontology/admin/place_TLM_librarianEmail -->

    <owl:AnnotationProperty rdf:about="http://purl.bdrc.io/ontology/admin/place_TLM_librarianEmail">
        <rdfs:label xml:lang="en">The librarian email is used to send requests to the library staff.</rdfs:label>
        <rdfs:label xml:lang="en">tlm librarian email</rdfs:label>
        <rdfs:range rdf:resource="http://www.w3.org/2001/XMLSchema#string"/>
        <rdfs:domain rdf:resource="http://purl.bdrc.io/ontology/Place"/>
    </owl:AnnotationProperty>
    


    <!-- http://purl.bdrc.io/ontology/admin/place_TLM_num -->

    <owl:AnnotationProperty rdf:about="http://purl.bdrc.io/ontology/admin/place_TLM_num">
        <rdfs:comment>The num attribute records the last RID suffix allocated for the Library. The num should be a 6 digit zero filled string initialized to &quot;000001&quot;.</rdfs:comment>
        <rdfs:label xml:lang="en">tlm num</rdfs:label>
        <rdfs:range rdf:resource="http://www.w3.org/2001/XMLSchema#string"/>
        <rdfs:domain rdf:resource="http://purl.bdrc.io/ontology/Place"/>
    </owl:AnnotationProperty>
    


    <!-- http://purl.bdrc.io/ontology/admin/place_TLM_taxonomy -->

    <owl:AnnotationProperty rdf:about="http://purl.bdrc.io/ontology/admin/place_TLM_taxonomy">
        <rdfs:comment xml:lang="en">Identifies a Taxonomy that specifies the Library&apos;s shelf classification. By convention the taxonomy should have maximum depth of 4 levels - this constraint allows for a manageable GUI design.</rdfs:comment>
        <rdfs:label xml:lang="en">TLM taxonomy</rdfs:label>
        <rdfs:range rdf:resource="http://purl.bdrc.io/ontology/Taxonomy"/>
        <rdfs:domain rdf:resource="http://purl.bdrc.io/ontology/Place"/>
    </owl:AnnotationProperty>
    


    <!-- http://purl.bdrc.io/ontology/admin/place_dist_py -->

    <owl:AnnotationProperty rdf:about="http://purl.bdrc.io/ontology/admin/place_dist_py">
        <rdfs:comment xml:lang="en">The name in Pinyin of the district containing this Place from import of historical places prepared by Karl Ryavec and Lex Berman.</rdfs:comment>
        <rdfs:label xml:lang="en">district</rdfs:label>
        <rdfs:range rdf:resource="http://www.w3.org/1999/02/22-rdf-syntax-ns#PlainLiteral"/>
        <rdfs:domain rdf:resource="http://purl.bdrc.io/ontology/Place"/>
    </owl:AnnotationProperty>
    


    <!-- http://purl.bdrc.io/ontology/admin/place_gb_dist -->

    <owl:AnnotationProperty rdf:about="http://purl.bdrc.io/ontology/admin/place_gb_dist">
        <rdfs:comment xml:lang="en">An old GB code for the district containing this place from import of historical Tibetan places by Karl Ryavec and Lex Beerman</rdfs:comment>
        <rdfs:label xml:lang="en">old containing district gb</rdfs:label>
        <rdfs:range rdf:resource="http://www.w3.org/2001/XMLSchema#string"/>
        <rdfs:domain rdf:resource="http://purl.bdrc.io/ontology/Place"/>
    </owl:AnnotationProperty>
    


    <!-- http://purl.bdrc.io/ontology/admin/place_gonpa_per1000 -->

    <owl:AnnotationProperty rdf:about="http://purl.bdrc.io/ontology/admin/place_gonpa_per1000">
        <rdfs:comment xml:lang="en">The number of monasteries per 1000 sq km in this Place (presumably a region) from data provided by Karl Ryavec</rdfs:comment>
        <rdfs:label xml:lang="en">monasteries per 1000 sq km</rdfs:label>
        <rdfs:range rdf:resource="http://www.w3.org/2001/XMLSchema#string"/>
        <rdfs:domain rdf:resource="http://purl.bdrc.io/ontology/Place"/>
    </owl:AnnotationProperty>
    


    <!-- http://purl.bdrc.io/ontology/admin/place_id_Lex -->

    <owl:AnnotationProperty rdf:about="http://purl.bdrc.io/ontology/admin/place_id_Lex">
        <rdfs:comment xml:lang="en">Place ID assigned by Lex Berman used for import of historical Tibetan place information. This id is based on an old GB code and is not current. It will be removed in the future from the data set</rdfs:comment>
        <rdfs:label xml:lang="en">place ID Lex</rdfs:label>
        <rdfs:range rdf:resource="http://www.w3.org/2001/XMLSchema#string"/>
        <rdfs:domain rdf:resource="http://purl.bdrc.io/ontology/Place"/>
    </owl:AnnotationProperty>
    


    <!-- http://purl.bdrc.io/ontology/admin/place_id_TBRC -->

    <owl:AnnotationProperty rdf:about="http://purl.bdrc.io/ontology/admin/place_id_TBRC">
        <rdfs:comment xml:lang="en">Place ID assigned by Karl Ryavec used for import of historical Tibetan place information. This id is based on an old GB code and is not current. It will be removed in the future from the data set</rdfs:comment>
        <rdfs:label xml:lang="en">place id TBRC</rdfs:label>
        <rdfs:range rdf:resource="http://www.w3.org/2001/XMLSchema#string"/>
        <rdfs:domain rdf:resource="http://purl.bdrc.io/ontology/Place"/>
    </owl:AnnotationProperty>
    


    <!-- http://purl.bdrc.io/ontology/admin/place_name_kr -->

    <owl:AnnotationProperty rdf:about="http://purl.bdrc.io/ontology/admin/place_name_kr">
        <rdfs:comment xml:lang="en">Place name provided by Karl Ryavec for import of historical Tibetan places</rdfs:comment>
        <rdfs:label xml:lang="en">name per KR</rdfs:label>
        <rdfs:range rdf:resource="http://www.w3.org/2001/XMLSchema#string"/>
        <rdfs:domain rdf:resource="http://purl.bdrc.io/ontology/Place"/>
    </owl:AnnotationProperty>
    


    <!-- http://purl.bdrc.io/ontology/admin/place_name_lex -->

    <owl:AnnotationProperty rdf:about="http://purl.bdrc.io/ontology/admin/place_name_lex">
        <rdfs:comment xml:lang="en">Place name provided by Lex Berman for import of historical Tibetan places</rdfs:comment>
        <rdfs:label xml:lang="en">name per lex</rdfs:label>
        <rdfs:range rdf:resource="http://www.w3.org/2001/XMLSchema#string"/>
        <rdfs:domain rdf:resource="http://purl.bdrc.io/ontology/Place"/>
    </owl:AnnotationProperty>
    


    <!-- http://purl.bdrc.io/ontology/admin/place_prov_py -->

    <owl:AnnotationProperty rdf:about="http://purl.bdrc.io/ontology/admin/place_prov_py">
        <rdfs:comment xml:lang="en">Name of containing province in pinyin per Karl Ryavec for import of historical places</rdfs:comment>
        <rdfs:label xml:lang="en">province name</rdfs:label>
        <rdfs:range rdf:resource="http://www.w3.org/1999/02/22-rdf-syntax-ns#PlainLiteral"/>
        <rdfs:domain rdf:resource="http://purl.bdrc.io/ontology/Place"/>
    </owl:AnnotationProperty>
    


    <!-- http://purl.bdrc.io/ontology/admin/place_town_ch -->

    <owl:AnnotationProperty rdf:about="http://purl.bdrc.io/ontology/admin/place_town_ch">
        <rdfs:comment xml:lang="en">Name of the containing town in Chinese unicode per Karl Ryavec for import of historical Tibetan places</rdfs:comment>
        <rdfs:label xml:lang="en">town name</rdfs:label>
        <rdfs:range rdf:resource="http://www.w3.org/1999/02/22-rdf-syntax-ns#PlainLiteral"/>
        <rdfs:domain rdf:resource="http://purl.bdrc.io/ontology/Place"/>
    </owl:AnnotationProperty>
    


    <!-- http://purl.bdrc.io/ontology/admin/place_town_py -->

    <owl:AnnotationProperty rdf:about="http://purl.bdrc.io/ontology/admin/place_town_py">
        <rdfs:comment xml:lang="en">Name of containing town in pinyin per Karl Ryavec for import of historical Tibetan places</rdfs:comment>
        <rdfs:label xml:lang="en">town name</rdfs:label>
        <rdfs:range rdf:resource="http://www.w3.org/1999/02/22-rdf-syntax-ns#PlainLiteral"/>
        <rdfs:domain rdf:resource="http://purl.bdrc.io/ontology/Place"/>
    </owl:AnnotationProperty>
    


    <!-- http://purl.bdrc.io/ontology/admin/place_town_syl -->

    <owl:AnnotationProperty rdf:about="http://purl.bdrc.io/ontology/admin/place_town_syl">
        <rdfs:comment xml:lang="en">Another version of the name of the containing town per Karl Ryavec</rdfs:comment>
        <rdfs:label xml:lang="en">town name</rdfs:label>
        <rdfs:range rdf:resource="http://www.w3.org/2001/XMLSchema#string"/>
        <rdfs:domain rdf:resource="http://purl.bdrc.io/ontology/Place"/>
    </owl:AnnotationProperty>
    


    <!-- http://purl.bdrc.io/ontology/admin/productAllowByAddr -->

    <owl:AnnotationProperty rdf:about="http://purl.bdrc.io/ontology/admin/productAllowByAddr">
        <rdfs:comment xml:lang="en">The prodcutAllowByAddr has an xsd:string with the format of a cidr IP address range, e.g., 128.2.8.0/24. These address ranges are used to permit access to collections of works</rdfs:comment>
        <rdfs:range rdf:resource="http://www.w3.org/2001/XMLSchema#string"/>
        <rdfs:domain rdf:resource="http://purl.bdrc.io/ontology/admin/ProductOrg"/>
    </owl:AnnotationProperty>
    


    <!-- http://purl.bdrc.io/ontology/admin/productIncludes -->

    <owl:AnnotationProperty rdf:about="http://purl.bdrc.io/ontology/admin/productIncludes">
        <rdfs:comment xml:lang="en">A Product may include another Product for the purpose of including access information in support of the subscription service.</rdfs:comment>
        <rdfs:label xml:lang="en">includes</rdfs:label>
        <rdfs:range rdf:resource="http://purl.bdrc.io/ontology/admin/Product"/>
        <rdfs:domain rdf:resource="http://purl.bdrc.io/ontology/admin/Product"/>
    </owl:AnnotationProperty>
    


    <!-- http://purl.bdrc.io/ontology/admin/volumeQcDate -->

    <owl:AnnotationProperty rdf:about="http://purl.bdrc.io/ontology/admin/volumeQcDate">
        <rdfs:range rdf:resource="http://www.w3.org/2001/XMLSchema#string"/>
        <rdfs:domain rdf:resource="http://purl.bdrc.io/ontology/Volume"/>
    </owl:AnnotationProperty>
    


    <!-- http://purl.bdrc.io/ontology/admin/volumeQcNote -->

    <owl:AnnotationProperty rdf:about="http://purl.bdrc.io/ontology/admin/volumeQcNote">
        <rdfs:range rdf:resource="http://www.w3.org/2001/XMLSchema#string"/>
        <rdfs:domain rdf:resource="http://purl.bdrc.io/ontology/Volume"/>
    </owl:AnnotationProperty>
    


    <!-- http://purl.bdrc.io/ontology/admin/volumeQcPerson -->

    <owl:AnnotationProperty rdf:about="http://purl.bdrc.io/ontology/admin/volumeQcPerson">
        <rdfs:range rdf:resource="http://www.w3.org/2001/XMLSchema#string"/>
        <rdfs:domain rdf:resource="http://purl.bdrc.io/ontology/Volume"/>
    </owl:AnnotationProperty>
    


    <!-- http://purl.bdrc.io/ontology/admin/volumeScanVenue -->

    <owl:AnnotationProperty rdf:about="http://purl.bdrc.io/ontology/admin/volumeScanVenue">
        <rdfs:comment xml:lang="en">this property is used to migrate the venue attribute from scanrequest. it records where the scanning was to take place</rdfs:comment>
        <rdfs:range rdf:resource="http://www.w3.org/2001/XMLSchema#string"/>
        <rdfs:domain rdf:resource="http://purl.bdrc.io/ontology/Item"/>
    </owl:AnnotationProperty>
    


    <!-- http://purl.bdrc.io/ontology/admin/workAccess -->

    <owl:AnnotationProperty rdf:about="http://purl.bdrc.io/ontology/admin/workAccess">
        <rdfs:comment xml:lang="en">The type of online access permitted for the subject Work.</rdfs:comment>
        <rdfs:label xml:lang="en">permitted access</rdfs:label>
        <rdfs:seeAlso rdf:resource="http://purl.bdrc.io/ontology/WorkAccessType"/>
        <rdfs:range rdf:resource="http://purl.bdrc.io/ontology/WorkAccessType"/>
        <rdfs:domain rdf:resource="http://purl.bdrc.io/ontology/Work"/>
    </owl:AnnotationProperty>
    


    <!-- http://purl.bdrc.io/ontology/admin/workLicense -->

    <owl:AnnotationProperty rdf:about="http://purl.bdrc.io/ontology/admin/workLicense">
        <rdfs:comment xml:lang="en">The license under which access to the Work is provided</rdfs:comment>
        <rdfs:label xml:lang="en">has license</rdfs:label>
        <rdfs:seeAlso rdf:resource="http://purl.bdrc.io/ontology/WorkLicense"/>
        <rdfs:range rdf:resource="http://purl.bdrc.io/ontology/WorkLicense"/>
        <rdfs:domain rdf:resource="http://purl.bdrc.io/ontology/Work"/>
    </owl:AnnotationProperty>
    


    <!-- http://purl.bdrc.io/ontology/admin/work_desc_date -->

    <owl:AnnotationProperty rdf:about="http://purl.bdrc.io/ontology/admin/work_desc_date">
        <rdfs:comment xml:lang="en">Migration hint: Used only in O01CT0001 to record some sort of date information from the colophons of various texts. The format is non-standard will require further examination</rdfs:comment>
        <rdfs:label xml:lang="en">date from description</rdfs:label>
        <rdfs:range rdf:resource="http://www.w3.org/2001/XMLSchema#string"/>
        <rdfs:domain rdf:resource="http://purl.bdrc.io/ontology/Work"/>
    </owl:AnnotationProperty>
    


    <!-- http://purl.org/dc/terms/modified -->

    <owl:AnnotationProperty rdf:about="http://purl.org/dc/terms/modified"/>
    


    <!-- http://www.w3.org/2000/01/rdf-schema#comment -->

    <rdf:Description rdf:about="http://www.w3.org/2000/01/rdf-schema#comment">
        <rdfs:label xml:lang="en">As a convention in the BDRC ontology, use rdfs:comment for summary and contents statements about a resource rather than adding additional properties.

We take the view that the summary or contents statements can be treated in a manner similar to the use of rdfs:label as a way of providing a short description of a resource</rdfs:label>
        <rdfs:label xml:lang="en">Migration hint: map &lt;?:description type=&quot;summary&quot;/&gt; and &lt;?:description type=&quot;contents&quot;/&gt; to rdfs:comment</rdfs:label>
    </rdf:Description>
    


    <!-- http://www.w3.org/2000/01/rdf-schema#label -->

    <rdf:Description rdf:about="http://www.w3.org/2000/01/rdf-schema#label">
        <rdfs:label xml:lang="en">The rdfs:label is used in the BDRC ontology to provide a preferred and localized human readable label for any resource. So while we provide :name to give all of the variants for a name or title for a Work, Person and so on</rdfs:label>
    </rdf:Description>
    


    <!-- 
    ///////////////////////////////////////////////////////////////////////////////////////
    //
    // Datatypes
    //
    ///////////////////////////////////////////////////////////////////////////////////////
     -->

    


    <!-- http://purl.bdrc.io/ontology/ISBN -->

    <rdfs:Datatype rdf:about="http://purl.bdrc.io/ontology/ISBN">
        <dataTypeExpression>^(97(8|9))?\d{9}(\d|X)$</dataTypeExpression>
        <rdfs:comment xml:lang="en">The regex is does not take into account opitional blank, &apos; &apos;, or dash, &apos;-&apos;, chars separating the various groups. Also there is no spec for calculating the check digit</rdfs:comment>
        <rdfs:isDefinedBy rdf:resource="https://www.isbn-international.org/sites/default/files/ISBN%20Manual%202012%20-corr.pdf"/>
        <rdfs:label xml:lang="en">International Standard Book Number</rdfs:label>
    </rdfs:Datatype>
    


    <!-- http://purl.bdrc.io/ontology/LCCN -->

    <rdfs:Datatype rdf:about="http://purl.bdrc.io/ontology/LCCN">
        <dataTypeExpression>[[a-z]|[[a-z][a-z]|dd]|[a-z][[a-z][a-z]|dd]|[a-z][a-z]dd]dddddddd</dataTypeExpression>
        <rdfs:isDefinedBy rdf:resource="http://www.loc.gov/marc/lccn-namespace.html"/>
        <rdfs:label xml:lang="en">Library of Congress Control Number</rdfs:label>
        <owl:equivalentClass rdf:resource="http://www.w3.org/2001/XMLSchema#string"/>
    </rdfs:Datatype>
    


    <!-- http://purl.bdrc.io/ontology/LCCallNumber -->

    <rdfs:Datatype rdf:about="http://purl.bdrc.io/ontology/LCCallNumber">
        <dataTypeExpression rdf:resource="https://gist.github.com/kurtraschke/560162"/>
        <rdfs:isDefinedBy rdf:resource="https://www.loc.gov/aba/publications/FreeCSM/freecsm.html"/>
        <rdfs:label xml:lang="en">Library of Congress Call Number</rdfs:label>
        <rdfs:seeAlso rdf:resource="https://www.loc.gov/catdir/cpso/lcco/"/>
    </rdfs:Datatype>
    


    <!-- http://purl.bdrc.io/ontology/StatusType -->

    <rdfs:Datatype rdf:about="http://purl.bdrc.io/ontology/StatusType">
        <owl:equivalentClass>
            <rdfs:Datatype>
                <owl:oneOf>
                    <rdf:Description>
                        <rdf:type rdf:resource="http://www.w3.org/1999/02/22-rdf-syntax-ns#List"/>
                        <rdf:first>accessioned</rdf:first>
                        <rdf:rest>
                            <rdf:Description>
                                <rdf:type rdf:resource="http://www.w3.org/1999/02/22-rdf-syntax-ns#List"/>
                                <rdf:first>acquiring</rdf:first>
                                <rdf:rest>
                                    <rdf:Description>
                                        <rdf:type rdf:resource="http://www.w3.org/1999/02/22-rdf-syntax-ns#List"/>
                                        <rdf:first>editing</rdf:first>
                                        <rdf:rest>
                                            <rdf:Description>
                                                <rdf:type rdf:resource="http://www.w3.org/1999/02/22-rdf-syntax-ns#List"/>
                                                <rdf:first>onHold</rdf:first>
                                                <rdf:rest>
                                                    <rdf:Description>
                                                        <rdf:type rdf:resource="http://www.w3.org/1999/02/22-rdf-syntax-ns#List"/>
                                                        <rdf:first>provisional</rdf:first>
                                                        <rdf:rest>
                                                            <rdf:Description>
                                                                <rdf:type rdf:resource="http://www.w3.org/1999/02/22-rdf-syntax-ns#List"/>
                                                                <rdf:first>released</rdf:first>
                                                                <rdf:rest>
                                                                    <rdf:Description>
                                                                        <rdf:type rdf:resource="http://www.w3.org/1999/02/22-rdf-syntax-ns#List"/>
                                                                        <rdf:first>scanned</rdf:first>
                                                                        <rdf:rest>
                                                                            <rdf:Description>
                                                                                <rdf:type rdf:resource="http://www.w3.org/1999/02/22-rdf-syntax-ns#List"/>
                                                                                <rdf:first>seekingOut</rdf:first>
                                                                                <rdf:rest>
                                                                                    <rdf:Description>
                                                                                        <rdf:type rdf:resource="http://www.w3.org/1999/02/22-rdf-syntax-ns#List"/>
                                                                                        <rdf:first>withdrawn</rdf:first>
                                                                                        <rdf:rest rdf:resource="http://www.w3.org/1999/02/22-rdf-syntax-ns#nil"/>
                                                                                    </rdf:Description>
                                                                                </rdf:rest>
                                                                            </rdf:Description>
                                                                        </rdf:rest>
                                                                    </rdf:Description>
                                                                </rdf:rest>
                                                            </rdf:Description>
                                                        </rdf:rest>
                                                    </rdf:Description>
                                                </rdf:rest>
                                            </rdf:Description>
                                        </rdf:rest>
                                    </rdf:Description>
                                </rdf:rest>
                            </rdf:Description>
                        </rdf:rest>
                    </rdf:Description>
                </owl:oneOf>
            </rdfs:Datatype>
        </owl:equivalentClass>
    </rdfs:Datatype>
    


    <!-- 
    ///////////////////////////////////////////////////////////////////////////////////////
    //
    // Object Properties
    //
    ///////////////////////////////////////////////////////////////////////////////////////
     -->

    


    <!-- http://id.loc.gov/ontologies/bibframe/identifiedBy -->

    <owl:ObjectProperty rdf:about="http://id.loc.gov/ontologies/bibframe/identifiedBy">
        <rdfs:subPropertyOf rdf:resource="http://id.loc.gov/ontologies/bibframe/objectProperty"/>
        <owl:inverseOf rdf:resource="http://id.loc.gov/ontologies/bibframe/identifies"/>
        <rdfs:domain rdf:resource="http://purl.bdrc.io/ontology/Work"/>
        <rdfs:range rdf:resource="http://id.loc.gov/ontologies/bibframe/Identifier"/>
    </owl:ObjectProperty>
    


    <!-- http://id.loc.gov/ontologies/bibframe/identifies -->

    <owl:ObjectProperty rdf:about="http://id.loc.gov/ontologies/bibframe/identifies">
        <rdfs:subPropertyOf rdf:resource="http://id.loc.gov/ontologies/bibframe/objectProperty"/>
    </owl:ObjectProperty>
    


    <!-- http://id.loc.gov/ontologies/bibframe/objectProperty -->

    <owl:ObjectProperty rdf:about="http://id.loc.gov/ontologies/bibframe/objectProperty"/>
    


    <!-- http://purl.bdrc.io/ontology/corporationHasMember -->

    <owl:ObjectProperty rdf:about="http://purl.bdrc.io/ontology/corporationHasMember">
        <rdfs:domain rdf:resource="http://purl.bdrc.io/ontology/Corporation"/>
        <rdfs:range rdf:resource="http://purl.bdrc.io/ontology/CorporationMember"/>
    </owl:ObjectProperty>
    


    <!-- http://purl.bdrc.io/ontology/corporationMember -->

    <owl:ObjectProperty rdf:about="http://purl.bdrc.io/ontology/corporationMember">
        <rdfs:domain rdf:resource="http://purl.bdrc.io/ontology/CorporationMember"/>
        <rdfs:range rdf:resource="http://purl.bdrc.io/ontology/Person"/>
        <inferSubTree rdf:datatype="http://www.w3.org/2001/XMLSchema#boolean">true</inferSubTree>
    </owl:ObjectProperty>
    


    <!-- http://purl.bdrc.io/ontology/corporationMemberType -->

    <owl:ObjectProperty rdf:about="http://purl.bdrc.io/ontology/corporationMemberType">
        <rdfs:domain rdf:resource="http://purl.bdrc.io/ontology/CorporationMember"/>
        <rdfs:range rdf:resource="http://purl.bdrc.io/ontology/CorporationMemberType"/>
    </owl:ObjectProperty>
    


    <!-- http://purl.bdrc.io/ontology/corporationRegion -->

    <owl:ObjectProperty rdf:about="http://purl.bdrc.io/ontology/corporationRegion">
        <rdfs:domain rdf:resource="http://purl.bdrc.io/ontology/Corporation"/>
        <rdfs:range rdf:resource="http://purl.bdrc.io/ontology/Place"/>
        <rdfs:comment xml:lang="en">
The original corporation.xsd includes several attributes on &lt;region/&gt;: @start, @startCirca, @end, @endCirca that are not used except in one case 
for @start, C71, and a different instance, C13, for @endCirca. The uses are not correct and these attributes have not been included in the current model.

Thus crp:region maps crp:Corporation directly to plc:Place without any additional chaff</rdfs:comment>
        <rdfs:comment xml:lang="en">This property records a Place characterizing the region in which the Corporation occured/occurs.</rdfs:comment>
    </owl:ObjectProperty>
    


    <!-- http://purl.bdrc.io/ontology/itemForWork -->

    <owl:ObjectProperty rdf:about="http://purl.bdrc.io/ontology/itemForWork">
        <owl:inverseOf rdf:resource="http://purl.bdrc.io/ontology/workHasItem"/>
        <rdfs:domain rdf:resource="http://purl.bdrc.io/ontology/Item"/>
        <rdfs:range rdf:resource="http://purl.bdrc.io/ontology/Work"/>
        <rdfs:comment xml:lang="en">This Item is for the referenced Work, i.e., this Item represents a physical or digital instance of the referenced Work</rdfs:comment>
        <rdfs:label xml:lang="en">for work</rdfs:label>
    </owl:ObjectProperty>
    


    <!-- http://purl.bdrc.io/ontology/itemHasVolume -->

    <owl:ObjectProperty rdf:about="http://purl.bdrc.io/ontology/itemHasVolume">
        <owl:inverseOf rdf:resource="http://purl.bdrc.io/ontology/volumeOf"/>
        <rdfs:domain rdf:resource="http://purl.bdrc.io/ontology/Item"/>
        <rdfs:range rdf:resource="http://purl.bdrc.io/ontology/Volume"/>
        <rdfs:comment xml:lang="en">refers to a volume description which could be a digital asset, scanned or etext; or a physical volume (part of a physical holding)</rdfs:comment>
        <rdfs:label xml:lang="en">has volume</rdfs:label>
    </owl:ObjectProperty>
    


    <!-- http://purl.bdrc.io/ontology/itemType -->

    <owl:ObjectProperty rdf:about="http://purl.bdrc.io/ontology/itemType">
        <rdfs:domain rdf:resource="http://purl.bdrc.io/ontology/Item"/>
        <rdfs:range rdf:resource="http://purl.bdrc.io/ontology/ItemType"/>
        <rdfs:comment xml:lang="en">Indicates the type of the Item: physical work, digital asset - scanned, ocr&apos;d or input.</rdfs:comment>
        <rdfs:comment xml:lang="en">Migration hint: imagegroups with lists of image names will be of type bdr:ItemTypeImageAsset</rdfs:comment>
        <rdfs:label xml:lang="en">item type</rdfs:label>
    </owl:ObjectProperty>
    


    <!-- http://purl.bdrc.io/ontology/lineageAlternative -->

    <owl:ObjectProperty rdf:about="http://purl.bdrc.io/ontology/lineageAlternative">
        <rdfs:domain rdf:resource="http://purl.bdrc.io/ontology/Lineage"/>
        <rdfs:range rdf:resource="http://purl.bdrc.io/ontology/LineageAlternative"/>
        <rdfs:seeAlso rdf:resource="http://purl.bdrc.io/ontology/LineageAlternative"/>
        <owl:deprecated xml:lang="en">deprecated. See :LineageAlternative for details</owl:deprecated>
    </owl:ObjectProperty>
    


    <!-- http://purl.bdrc.io/ontology/lineageDownFrom -->

    <owl:ObjectProperty rdf:about="http://purl.bdrc.io/ontology/lineageDownFrom">
        <rdfs:domain rdf:resource="http://purl.bdrc.io/ontology/LineageHolder"/>
        <rdfs:range rdf:resource="http://purl.bdrc.io/ontology/Lineage"/>
        <rdfs:comment xml:lang="en">This models the &quot;down from ...&quot; references to other Lineages. The :Lineage object of :lineageDownFrom will contain the same :LineageHolder as here and the meaning of :lineageDownFrom is to &quot;splice&quot; the remaining holders on to the end of this lineage.

This models the directly the way in which the source gsan/thob yigs are written.

For example, here is the &quot;tail&quot; of bdr:L0RKL137:

bdr:L0RKL137 a :Lineage ;
      :lineageType bdr:LineageDbang ;
      :lineageObject bdr:T976 ;
. . .
      :lineageHolder [ a :LineageHolder ;
            :lineageWho bdr:P502 ;
            :lineageReceived [ a :LineageReceived ;
                  :lineageFrom bdr:P1226 ]
            ]
      :lineageHolder [ a :LineageHolder ;
            :lineageWho bdr:P3094 ;
            :lineageReceived [ a :LineageReceived ;
                  :lineageFrom bdr:P502 ]
            :lineageDownFrom bdr:L0RKL134
            ]

Now in bdr:L0RKL134 there will be found a :LineageHolder with a :lineageWho of bdr:P3094 and all of the holders from then to the end of bdr:L0RKL134 are considered to be appended to bdr:L0RKL137:

bdr:L0RKL134 a :Lineage ;
      :lineageType bdr:LineageDbang ;
      :lineageObject bdr:T976 ;
. . .
      :lineageHolder [ a :LineageHolder ;
            :lineageWho bdr:P502 ;
            :lineageReceived [ a :LineageReceived ;
                  :lineageFrom bdr:P3093 ]
            ]
      :lineageHolder [ a :LineageHolder ;
            :lineageWho bdr:P3094 ;
            :lineageReceived [ a :LineageReceived ;
                  :lineageFrom bdr:P502 ]
            ]
      :lineageHolder [ a :LineageHolder ;
            :lineageWho bdr:P1132 ;
            :lineageReceived [ a :LineageReceived ;
                  :lineageFrom bdr:P3094 ]
            ]
      :lineageHolder [ a :LineageHolder ;
            :lineageWho bdr:P1034 ;
            :lineageReceived [ a :LineageReceived ;
                  :lineageFrom bdr:P1132 ]
            ]
. . .

This illustrates that while bdr:P3094 received the :Lineage from bdr:P502 in both cases, bdr:P502 received the lineage from bdr:P3093 in one case and from bdr:P1226 in the other. The two :Lineages are both of the same type and are transmitting the same object, bdr:T976, so this example illustrates the use of :lineageDownFrom to simplify the recording in a gsan yig or thob yig while highlighting some of the commonalities.</rdfs:comment>
        <rdfs:label xml:lang="en">down from</rdfs:label>
        <rdfs:seeAlso rdf:resource="http://purl.bdrc.io/ontology/LineageHolder"/>
    </owl:ObjectProperty>
    


    <!-- http://purl.bdrc.io/ontology/lineageDownTo -->

    <owl:ObjectProperty rdf:about="http://purl.bdrc.io/ontology/lineageDownTo">
        <rdfs:domain rdf:resource="http://purl.bdrc.io/ontology/LineageHolder"/>
        <rdfs:range rdf:resource="http://purl.bdrc.io/ontology/Lineage"/>
        <rdfs:comment xml:lang="en">This models the &quot;down to ...&quot; references to other Lineages. The other Lineage from the beginning to the holder with the same who as this holder is implicitly included with this lineage. The known use case is for the initial holder to include the prior holders from another lineage as the initial without having members of this lineage without having to repeat them. It may be meaningful to use this feature deeper in a lineage but that is not defined at this time. It is meaningful to include multiple from references which is interpreted as implicitly creating an alternative lineage for each from element.</rdfs:comment>
        <rdfs:label xml:lang="en">down to</rdfs:label>
        <rdfs:seeAlso rdf:resource="http://purl.bdrc.io/ontology/LineageHolder"/>
        <rdfs:seeAlso rdf:resource="http://purl.bdrc.io/ontology/lineageDownFrom"/>
    </owl:ObjectProperty>
    


    <!-- http://purl.bdrc.io/ontology/lineageFrom -->

    <owl:ObjectProperty rdf:about="http://purl.bdrc.io/ontology/lineageFrom">
        <rdfs:domain rdf:resource="http://purl.bdrc.io/ontology/LineageReceived"/>
        <rdfs:range>
            <owl:Class>
                <owl:unionOf rdf:parseType="Collection">
                    <rdf:Description rdf:about="http://purl.bdrc.io/ontology/Person"/>
                    <rdf:Description rdf:about="http://purl.bdrc.io/ontology/Topic"/>
                </owl:unionOf>
            </owl:Class>
        </rdfs:range>
        <rdfs:comment>Range should be unionOf Person and Deity(Topics)</rdfs:comment>
        <rdfs:comment xml:lang="en">Who did this &quot;LineageHolder receive the :Lineage from?</rdfs:comment>
        <rdfs:comment>original XSD has &quot;RID&quot; attr in &quot;Received&quot;</rdfs:comment>
        <rdfs:label xml:lang="en">received from</rdfs:label>
        <rdfs:seeAlso rdf:resource="http://purl.bdrc.io/ontology/LineageReceived"/>
    </owl:ObjectProperty>
    


    <!-- http://purl.bdrc.io/ontology/lineageHolder -->

    <owl:ObjectProperty rdf:about="http://purl.bdrc.io/ontology/lineageHolder">
        <rdfs:domain rdf:resource="http://purl.bdrc.io/ontology/Lineage"/>
        <rdfs:range rdf:resource="http://purl.bdrc.io/ontology/LineageHolder"/>
        <rdfs:comment xml:lang="en">the object of :lineageHolder is a :LineageHolder that describes an individual that held the given :Lineage</rdfs:comment>
        <rdfs:label xml:lang="en">has holder</rdfs:label>
        <rdfs:seeAlso rdf:resource="http://purl.bdrc.io/ontology/LineageHolder"/>
    </owl:ObjectProperty>
    


    <!-- http://purl.bdrc.io/ontology/lineageObject -->

    <owl:ObjectProperty rdf:about="http://purl.bdrc.io/ontology/lineageObject">
        <rdfs:domain rdf:resource="http://purl.bdrc.io/ontology/Lineage"/>
        <rdfs:range rdf:resource="http://purl.bdrc.io/ontology/Entity"/>
        <rdfs:comment xml:lang="en">This is a reference to what is being transmitted in the :Lineage. Typically this is a deity, ritual, or teaching or some sort. The :lineageType will indicate the nature of the :Lineage transmission, empowerment, reading transmission, instructions on practice and so on.

The object should be restricted to Persons or to Topics that represent a Deity or other suitable objects of a Lineage (what might those be?). This requires a union of some sort.</rdfs:comment>
        <rdfs:label xml:lang="en">transmits</rdfs:label>
        <rdfs:seeAlso rdf:resource="http://purl.bdrc.io/ontology/Lineage"/>
    </owl:ObjectProperty>
    


    <!-- http://purl.bdrc.io/ontology/lineageReceived -->

    <owl:ObjectProperty rdf:about="http://purl.bdrc.io/ontology/lineageReceived">
        <rdfs:domain rdf:resource="http://purl.bdrc.io/ontology/LineageHolder"/>
        <rdfs:range rdf:resource="http://purl.bdrc.io/ontology/LineageReceived"/>
        <rdfs:comment xml:lang="en">Essentially who did the holder receive this :Lineage from</rdfs:comment>
        <rdfs:label xml:lang="en">lineage received</rdfs:label>
        <rdfs:seeAlso rdf:resource="http://purl.bdrc.io/ontology/LineageReceived"/>
    </owl:ObjectProperty>
    


    <!-- http://purl.bdrc.io/ontology/lineageRef -->

    <owl:ObjectProperty rdf:about="http://purl.bdrc.io/ontology/lineageRef">
        <rdfs:domain rdf:resource="http://purl.bdrc.io/ontology/Lineage"/>
        <rdfs:range rdf:resource="http://purl.bdrc.io/ontology/Lineage"/>
        <rdfs:comment xml:lang="en">The :lineageRef identifies another :Lineage that is an alternative version of the current :Lineage. In gsan yig and thob yig there can be references to different versions of how a given object has been transmitted up to the time of the writing of the gsan/thob yig.</rdfs:comment>
        <rdfs:label xml:lang="en">alternative lineage</rdfs:label>
        <rdfs:seeAlso rdf:resource="http://purl.bdrc.io/ontology/Lineage"/>
    </owl:ObjectProperty>
    


    <!-- http://purl.bdrc.io/ontology/lineageSite -->

    <owl:ObjectProperty rdf:about="http://purl.bdrc.io/ontology/lineageSite">
        <rdfs:domain rdf:resource="http://purl.bdrc.io/ontology/LineageReceived"/>
        <rdfs:range rdf:resource="http://purl.bdrc.io/ontology/Place"/>
        <rdfs:comment>where the receiving occurred</rdfs:comment>
        <rdfs:seeAlso rdf:resource="http://purl.bdrc.io/ontology/LineageReceived"/>
    </owl:ObjectProperty>
    


    <!-- http://purl.bdrc.io/ontology/lineageType -->

    <owl:ObjectProperty rdf:about="http://purl.bdrc.io/ontology/lineageType">
        <rdf:type rdf:resource="http://www.w3.org/2002/07/owl#FunctionalProperty"/>
        <rdfs:domain rdf:resource="http://purl.bdrc.io/ontology/Lineage"/>
        <rdfs:range rdf:resource="http://purl.bdrc.io/ontology/LineageType"/>
        <rdfs:comment xml:lang="en">Identifies the type of :Lineage such as empowerment, reading transmission, various sorts of instructions and so on</rdfs:comment>
        <rdfs:label xml:lang="en">lineage type</rdfs:label>
        <rdfs:seeAlso rdf:resource="http://purl.bdrc.io/ontology/Lineage"/>
    </owl:ObjectProperty>
    


    <!-- http://purl.bdrc.io/ontology/lineageWho -->

    <owl:ObjectProperty rdf:about="http://purl.bdrc.io/ontology/lineageWho">
        <rdfs:domain rdf:resource="http://purl.bdrc.io/ontology/LineageHolder"/>
        <rdfs:range>
            <owl:Class>
                <owl:unionOf rdf:parseType="Collection">
                    <rdf:Description rdf:about="http://purl.bdrc.io/ontology/Person"/>
                    <rdf:Description rdf:about="http://purl.bdrc.io/ontology/Topic"/>
                </owl:unionOf>
            </owl:Class>
        </rdfs:range>
        <rdfs:comment xml:lang="en">identifies who this :LineageHolder is, :Person or a being represented via a :Topic.</rdfs:comment>
        <rdfs:label xml:lang="en">is holder</rdfs:label>
        <rdfs:seeAlso rdf:resource="http://purl.bdrc.io/ontology/LineageHolder"/>
    </owl:ObjectProperty>
    


    <!-- http://purl.bdrc.io/ontology/lineageWork -->

    <owl:ObjectProperty rdf:about="http://purl.bdrc.io/ontology/lineageWork">
        <rdfs:domain rdf:resource="http://purl.bdrc.io/ontology/LineageHolder"/>
        <rdfs:range rdf:resource="http://purl.bdrc.io/ontology/Work"/>
        <rdfs:comment xml:lang="en">This refers to a :Work that the subject :LineageHolder authored as an element of the :Lineage - a commentary of some sort typically</rdfs:comment>
        <rdfs:label xml:lang="en">work</rdfs:label>
        <rdfs:seeAlso rdf:resource="http://purl.bdrc.io/ontology/LineageHolder"/>
    </owl:ObjectProperty>
    


    <!-- http://purl.bdrc.io/ontology/personEvent -->

    <owl:ObjectProperty rdf:about="http://purl.bdrc.io/ontology/personEvent">
        <rdfs:domain rdf:resource="http://purl.bdrc.io/ontology/Person"/>
        <rdfs:range rdf:resource="http://purl.bdrc.io/ontology/PersonEvent"/>
        <rdfs:comment xml:lang="en">The source person.xsd includes event/pid which is not used and should be silently discarded during migration.</rdfs:comment>
        <rdfs:label xml:lang="en">event</rdfs:label>
    </owl:ObjectProperty>
    


    <!-- http://purl.bdrc.io/ontology/personEventCorporation -->

    <owl:ObjectProperty rdf:about="http://purl.bdrc.io/ontology/personEventCorporation">
        <rdfs:domain rdf:resource="http://purl.bdrc.io/ontology/PersonEvent"/>
        <rdfs:range rdf:resource="http://purl.bdrc.io/ontology/Corporation"/>
    </owl:ObjectProperty>
    


    <!-- http://purl.bdrc.io/ontology/personEventPlace -->

    <owl:ObjectProperty rdf:about="http://purl.bdrc.io/ontology/personEventPlace">
        <rdfs:domain rdf:resource="http://purl.bdrc.io/ontology/PersonEvent"/>
        <rdfs:range rdf:resource="http://purl.bdrc.io/ontology/Place"/>
        <rdfs:comment xml:lang="en">The place where the event took place</rdfs:comment>
        <rdfs:label xml:lang="en">place</rdfs:label>
    </owl:ObjectProperty>
    


    <!-- http://purl.bdrc.io/ontology/personEventRole -->

    <owl:ObjectProperty rdf:about="http://purl.bdrc.io/ontology/personEventRole">
        <rdfs:domain rdf:resource="http://purl.bdrc.io/ontology/PersonEvent"/>
        <rdfs:range rdf:resource="http://purl.bdrc.io/ontology/Role"/>
    </owl:ObjectProperty>
    


    <!-- http://purl.bdrc.io/ontology/personEventType -->

    <owl:ObjectProperty rdf:about="http://purl.bdrc.io/ontology/personEventType">
        <rdf:type rdf:resource="http://www.w3.org/2002/07/owl#FunctionalProperty"/>
        <rdfs:domain rdf:resource="http://purl.bdrc.io/ontology/PersonEvent"/>
        <rdfs:range rdf:resource="http://purl.bdrc.io/ontology/PersonEventType"/>
    </owl:ObjectProperty>
    


    <!-- http://purl.bdrc.io/ontology/personGender -->

    <owl:ObjectProperty rdf:about="http://purl.bdrc.io/ontology/personGender">
        <rdfs:domain rdf:resource="http://purl.bdrc.io/ontology/Person"/>
        <rdfs:range rdf:resource="http://purl.bdrc.io/ontology/Gender"/>
        <rdfs:label xml:lang="en">gender</rdfs:label>
    </owl:ObjectProperty>
    


    <!-- http://purl.bdrc.io/ontology/personHasConsort -->

    <owl:ObjectProperty rdf:about="http://purl.bdrc.io/ontology/personHasConsort">
        <rdfs:domain rdf:resource="http://purl.bdrc.io/ontology/Person"/>
        <rdfs:range rdf:resource="http://purl.bdrc.io/ontology/Person"/>
    </owl:ObjectProperty>
    


    <!-- http://purl.bdrc.io/ontology/personIncarnationOf -->

    <owl:ObjectProperty rdf:about="http://purl.bdrc.io/ontology/personIncarnationOf">
        <rdfs:domain rdf:resource="http://purl.bdrc.io/ontology/PersonIncarnationOf"/>
        <rdfs:range>
            <owl:Class>
                <owl:unionOf rdf:parseType="Collection">
                    <rdf:Description rdf:about="http://purl.bdrc.io/ontology/Person"/>
                    <rdf:Description rdf:about="http://purl.bdrc.io/ontology/Topic"/>
                </owl:unionOf>
            </owl:Class>
        </rdfs:range>
        <rdfs:comment xml:lang="en">Refers to the Person or Being (Topic) that this Person is an incarnation of</rdfs:comment>
        <rdfs:label xml:lang="en">incarnation of</rdfs:label>
    </owl:ObjectProperty>
    


    <!-- http://purl.bdrc.io/ontology/personIncarnationOfType -->

    <owl:ObjectProperty rdf:about="http://purl.bdrc.io/ontology/personIncarnationOfType">
        <rdfs:domain rdf:resource="http://purl.bdrc.io/ontology/PersonIncarnationOf"/>
        <rdfs:range rdf:resource="http://purl.bdrc.io/ontology/PersonIncarnationType"/>
        <rdfs:comment xml:lang="en">The type of incarnation: body, speech, mind and so on. On some occasions an individual may be recognized as more than one type of incarnation of the same individual in which case multiple occurrences of this property may be used.</rdfs:comment>
        <rdfs:label xml:lang="en">incarnation type</rdfs:label>
    </owl:ObjectProperty>
    


    <!-- http://purl.bdrc.io/ontology/personIsIncarnation -->

    <owl:ObjectProperty rdf:about="http://purl.bdrc.io/ontology/personIsIncarnation">
        <rdfs:domain rdf:resource="http://purl.bdrc.io/ontology/Person"/>
        <rdfs:range rdf:resource="http://purl.bdrc.io/ontology/PersonIncarnationOf"/>
        <rdfs:comment xml:lang="en">personIsIncarnation records which being (Person or Topic) this individual is an incarnation of and optionally what sort of incarnation (body speech, mind, etc). There are 1,456 individuals out of 18,320, that are marked as being incarnations of some being. Of these, 18 are marked with per:incarnationOf_relation and 5 are marked with per:incarnationOf_secondary.</rdfs:comment>
        <rdfs:label xml:lang="en">is incarnation</rdfs:label>
    </owl:ObjectProperty>
    


    <!-- http://purl.bdrc.io/ontology/personKin -->

    <owl:ObjectProperty rdf:about="http://purl.bdrc.io/ontology/personKin">
        <rdfs:domain rdf:resource="http://purl.bdrc.io/ontology/Person"/>
        <rdfs:range rdf:resource="http://purl.bdrc.io/ontology/Kin"/>
        <inferSubTree rdf:datatype="http://www.w3.org/2001/XMLSchema#boolean">true</inferSubTree>
        <rdfs:comment xml:lang="en">Associates a Person with another Person that they are kin to along with the type of the relation: mother, brother, etc.</rdfs:comment>
    </owl:ObjectProperty>
    


    <!-- http://purl.bdrc.io/ontology/personKinType -->

    <owl:ObjectProperty rdf:about="http://purl.bdrc.io/ontology/personKinType">
        <rdf:type rdf:resource="http://www.w3.org/2002/07/owl#FunctionalProperty"/>
        <rdfs:domain rdf:resource="http://purl.bdrc.io/ontology/Kin"/>
        <rdfs:range rdf:resource="http://purl.bdrc.io/ontology/KinType"/>
        <rdfs:label xml:lang="en">The KinType of the relation between the subject person and the referenced person</rdfs:label>
        <rdfs:label xml:lang="en">type</rdfs:label>
    </owl:ObjectProperty>
    


    <!-- http://purl.bdrc.io/ontology/personKinWho -->

    <owl:ObjectProperty rdf:about="http://purl.bdrc.io/ontology/personKinWho">
        <rdf:type rdf:resource="http://www.w3.org/2002/07/owl#FunctionalProperty"/>
        <rdfs:domain rdf:resource="http://purl.bdrc.io/ontology/Kin"/>
        <rdfs:range rdf:resource="http://purl.bdrc.io/ontology/Person"/>
        <rdfs:comment xml:lang="en">The referenced person in a kinship relation with the subject person</rdfs:comment>
        <rdfs:label xml:lang="en">who</rdfs:label>
    </owl:ObjectProperty>
    


    <!-- http://purl.bdrc.io/ontology/personName -->

    <owl:ObjectProperty rdf:about="http://purl.bdrc.io/ontology/personName">
        <rdf:type rdf:resource="http://www.w3.org/2002/07/owl#IrreflexiveProperty"/>
        <rdfs:domain rdf:resource="http://purl.bdrc.io/ontology/Person"/>
        <rdfs:range rdf:resource="http://purl.bdrc.io/ontology/PersonName"/>
        <rdfs:comment xml:lang="en">describe a name for a Person. Needed to include the type of the name as well as the rdf:LangString value for the name</rdfs:comment>
        <rdfs:label xml:lang="en">has name</rdfs:label>
    </owl:ObjectProperty>
    


    <!-- http://purl.bdrc.io/ontology/personNameType -->

    <owl:ObjectProperty rdf:about="http://purl.bdrc.io/ontology/personNameType">
        <rdfs:domain rdf:resource="http://purl.bdrc.io/ontology/PersonName"/>
        <rdfs:range rdf:resource="http://purl.bdrc.io/ontology/PersonNameType"/>
        <rdfs:comment xml:lang="en">the type of name described by the PersonName such as primary, first ordination, etc.</rdfs:comment>
        <rdfs:label xml:lang="en">type</rdfs:label>
    </owl:ObjectProperty>
    


    <!-- http://purl.bdrc.io/ontology/personOfSect -->

    <owl:ObjectProperty rdf:about="http://purl.bdrc.io/ontology/personOfSect">
        <rdfs:domain rdf:resource="http://purl.bdrc.io/ontology/Person"/>
        <rdfs:range rdf:resource="http://purl.bdrc.io/ontology/Topic"/>
    </owl:ObjectProperty>
    


    <!-- http://purl.bdrc.io/ontology/personStudentOf -->

    <owl:ObjectProperty rdf:about="http://purl.bdrc.io/ontology/personStudentOf">
        <owl:inverseOf rdf:resource="http://purl.bdrc.io/ontology/personTeacherOf"/>
        <rdfs:domain rdf:resource="http://purl.bdrc.io/ontology/Person"/>
        <rdfs:range rdf:resource="http://purl.bdrc.io/ontology/Person"/>
    </owl:ObjectProperty>
    


    <!-- http://purl.bdrc.io/ontology/personTeacherOf -->

    <owl:ObjectProperty rdf:about="http://purl.bdrc.io/ontology/personTeacherOf"/>
    


    <!-- http://purl.bdrc.io/ontology/placeAddress -->

    <owl:ObjectProperty rdf:about="http://purl.bdrc.io/ontology/placeAddress">
        <rdfs:domain rdf:resource="http://purl.bdrc.io/ontology/Place"/>
        <rdfs:range rdf:resource="http://purl.bdrc.io/ontology/PlaceAddress"/>
        <rdfs:comment xml:lang="en">Associates modern address information with a Place</rdfs:comment>
        <rdfs:label xml:lang="en">address</rdfs:label>
    </owl:ObjectProperty>
    


    <!-- http://purl.bdrc.io/ontology/placeContains -->

    <owl:ObjectProperty rdf:about="http://purl.bdrc.io/ontology/placeContains">
        <owl:inverseOf rdf:resource="http://purl.bdrc.io/ontology/placeLocatedIn"/>
        <rdfs:domain rdf:resource="http://purl.bdrc.io/ontology/Place"/>
        <rdfs:range rdf:resource="http://purl.bdrc.io/ontology/Place"/>
        <rdfs:comment xml:lang="en">Identifies a Place that this Place contains.</rdfs:comment>
        <rdfs:label xml:lang="en">contains</rdfs:label>
    </owl:ObjectProperty>
    


    <!-- http://purl.bdrc.io/ontology/placeEvent -->

    <owl:ObjectProperty rdf:about="http://purl.bdrc.io/ontology/placeEvent">
        <rdfs:domain rdf:resource="http://purl.bdrc.io/ontology/Place"/>
        <rdfs:range rdf:resource="http://purl.bdrc.io/ontology/PlaceEvent"/>
        <rdfs:comment xml:lang="en">Identifies an event that occurred at this Place, e.g., founded, rebuilt, deserted, etc.</rdfs:comment>
        <rdfs:label xml:lang="en">event</rdfs:label>
    </owl:ObjectProperty>
    


    <!-- http://purl.bdrc.io/ontology/placeEventAffiliation -->

    <owl:ObjectProperty rdf:about="http://purl.bdrc.io/ontology/placeEventAffiliation">
        <rdfs:domain rdf:resource="http://purl.bdrc.io/ontology/PlaceEvent"/>
        <rdfs:range rdf:resource="http://purl.bdrc.io/ontology/Tradition"/>
        <rdfs:comment xml:lang="en">Refers to the Tradition that the place event is affiliated with.</rdfs:comment>
        <rdfs:label xml:lang="en">affiliated tradition</rdfs:label>
    </owl:ObjectProperty>
    


    <!-- http://purl.bdrc.io/ontology/placeEventType -->

    <owl:ObjectProperty rdf:about="http://purl.bdrc.io/ontology/placeEventType">
        <rdfs:domain rdf:resource="http://purl.bdrc.io/ontology/PlaceEvent"/>
        <rdfs:range rdf:resource="http://purl.bdrc.io/ontology/PlaceEventType"/>
        <rdfs:comment xml:lang="en">The type of the Place event: founded, abandonded converted, etc</rdfs:comment>
        <rdfs:label xml:lang="en">event type</rdfs:label>
    </owl:ObjectProperty>
    


    <!-- http://purl.bdrc.io/ontology/placeIsNear -->

    <owl:ObjectProperty rdf:about="http://purl.bdrc.io/ontology/placeIsNear">
        <rdf:type rdf:resource="http://www.w3.org/2002/07/owl#SymmetricProperty"/>
        <rdfs:domain rdf:resource="http://purl.bdrc.io/ontology/Place"/>
        <rdfs:range rdf:resource="http://purl.bdrc.io/ontology/Place"/>
        <rdfs:comment xml:lang="en">Indicates that this Place is near to another - typically because of some reference in a document. In other words, there is some textual reason for mentioning the nearness; otherwise, the metadata could be filled with gratuitous nearness assertions.</rdfs:comment>
    </owl:ObjectProperty>
    


    <!-- http://purl.bdrc.io/ontology/placeLocatedIn -->

    <owl:ObjectProperty rdf:about="http://purl.bdrc.io/ontology/placeLocatedIn">
        <rdfs:domain rdf:resource="http://purl.bdrc.io/ontology/Place"/>
        <rdfs:range rdf:resource="http://purl.bdrc.io/ontology/Place"/>
        <rdfs:comment xml:lang="en">Identifies a Place that this Place is located in - usually a single Place but to account for changes over time in the definitions of regions and such it may be necessary to have multiple associations.</rdfs:comment>
        <rdfs:label xml:lang="en">located in</rdfs:label>
    </owl:ObjectProperty>
    


    <!-- http://purl.bdrc.io/ontology/placeType -->

    <owl:ObjectProperty rdf:about="http://purl.bdrc.io/ontology/placeType">
        <rdfs:domain rdf:resource="http://purl.bdrc.io/ontology/Place"/>
        <rdfs:range rdf:resource="http://purl.bdrc.io/ontology/PlaceType"/>
        <rdfs:comment xml:lang="en">The type of Place: monastery, river, mountain pass, etc.</rdfs:comment>
        <rdfs:label xml:lang="en">type</rdfs:label>
    </owl:ObjectProperty>
    


    <!-- http://purl.bdrc.io/ontology/taxElementOf -->

    <owl:ObjectProperty rdf:about="http://purl.bdrc.io/ontology/taxElementOf">
        <rdfs:domain rdf:resource="http://www.w3.org/2002/07/owl#Thing"/>
        <rdfs:range rdf:resource="http://www.w3.org/2002/07/owl#Thing"/>
        <rdfs:comment xml:lang="en">This property is used to indicated that a given Thing, usually some sort of Type, is an element of a (sub)class of some Taxonomy. The object of the property is typically some other individual of the same Type that is marked as a taxSubClassOf a Taxonomy or a (sub)class of a Taxonomy, etc.</rdfs:comment>
        <rdfs:label xml:lang="en">taxonomy element</rdfs:label>
    </owl:ObjectProperty>
    


    <!-- http://purl.bdrc.io/ontology/taxSubClass -->

    <owl:ObjectProperty rdf:about="http://purl.bdrc.io/ontology/taxSubClass">
        <rdfs:label xml:lang="en">This property identifies the subject as a subclass of a Taxonomy or some other subclass of a Taxonomy</rdfs:label>
        <rdfs:label xml:lang="en">taxonomy subclass</rdfs:label>
    </owl:ObjectProperty>
    


    <!-- http://purl.bdrc.io/ontology/volumeOf -->

    <owl:ObjectProperty rdf:about="http://purl.bdrc.io/ontology/volumeOf">
        <rdfs:domain rdf:resource="http://purl.bdrc.io/ontology/Volume"/>
        <rdfs:range rdf:resource="http://purl.bdrc.io/ontology/Item"/>
        <rdfs:comment xml:lang="en">The subject is a volume of the referenced item.</rdfs:comment>
        <rdfs:label xml:lang="en">volume of</rdfs:label>
    </owl:ObjectProperty>
    


    <!-- http://purl.bdrc.io/ontology/workCreator -->

    <owl:ObjectProperty rdf:about="http://purl.bdrc.io/ontology/workCreator">
        <rdfs:domain rdf:resource="http://purl.bdrc.io/ontology/Work"/>
        <rdfs:range rdf:resource="http://purl.bdrc.io/ontology/WorkCreator"/>
        <inferSubTree rdf:datatype="http://www.w3.org/2001/XMLSchema#boolean">true</inferSubTree>
        <rdfs:comment xml:lang="en">Identifies the type and person that are a creator of the work</rdfs:comment>
        <rdfs:label xml:lang="en">has creator</rdfs:label>
    </owl:ObjectProperty>
    


    <!-- http://purl.bdrc.io/ontology/workCreatorType -->

    <owl:ObjectProperty rdf:about="http://purl.bdrc.io/ontology/workCreatorType">
        <rdfs:domain rdf:resource="http://purl.bdrc.io/ontology/WorkCreator"/>
        <rdfs:range rdf:resource="http://purl.bdrc.io/ontology/WorkCreatorType"/>
        <rdfs:comment xml:lang="en">The type of the Work creator, e.g., main author, commentator, scribe, etc.</rdfs:comment>
        <rdfs:label xml:lang="en">has creator type</rdfs:label>
    </owl:ObjectProperty>
    


    <!-- http://purl.bdrc.io/ontology/workCreatorWho -->

    <owl:ObjectProperty rdf:about="http://purl.bdrc.io/ontology/workCreatorWho">
        <rdfs:domain rdf:resource="http://purl.bdrc.io/ontology/WorkCreator"/>
        <rdfs:range rdf:resource="http://purl.bdrc.io/ontology/Person"/>
        <rdfs:comment xml:lang="en">The :Person who is the creator of the :Work</rdfs:comment>
        <rdfs:label xml:lang="en">who</rdfs:label>
    </owl:ObjectProperty>
    


    <!-- http://purl.bdrc.io/ontology/workDerivativeOf -->

    <owl:ObjectProperty rdf:about="http://purl.bdrc.io/ontology/workDerivativeOf">
        <owl:inverseOf rdf:resource="http://purl.bdrc.io/ontology/workHasDerivative"/>
        <rdfs:domain rdf:resource="http://purl.bdrc.io/ontology/Work"/>
        <rdfs:range rdf:resource="http://purl.bdrc.io/ontology/Work"/>
        <rdfs:comment xml:lang="en">This work is a derivative of the reference work. This means that it may be a later edition or a version with some &quot;corrections&quot;/changes to the content of the referenced work.

For example,

bdr:W30532 :workDerivativeOf bdr:W22084

bdr:W30532 is a printing based on woodblocks that have a variety of &quot;corrections&quot; made via plugs in the original woodblocks and W22084 is a printing from the original sde dge Kanjur woodblocks so it makes sense to indicate that bdr:W30532 is a derivative of bdr:W22084.</rdfs:comment>
        <rdfs:label xml:lang="en">derivative of</rdfs:label>
    </owl:ObjectProperty>
    


    <!-- http://purl.bdrc.io/ontology/workExpressionOf -->

    <owl:ObjectProperty rdf:about="http://purl.bdrc.io/ontology/workExpressionOf">
        <owl:inverseOf rdf:resource="http://purl.bdrc.io/ontology/workHasExpression"/>
        <rdfs:domain rdf:resource="http://purl.bdrc.io/ontology/Work"/>
        <rdfs:range rdf:resource="http://purl.bdrc.io/ontology/Work"/>
        <rdfs:comment xml:lang="en">Migration info: The &lt;work:info @parent/&gt; should be migrated as :workExpressionOf</rdfs:comment>
        <rdfs:comment xml:lang="en">The subject work is an expression of the referenced work. This may mean that the subject work is an edition or version or the only extant occurrence of the referenced work.

This modeling is relevant when there are more than one occurrence of a work that needs to be accounted for in the library. If there is a single edition of a unique work then this elaborate modeling is not needed; however, for many works in the domain of Buddhist Universal Digital Archive there are many expressions of a single identified &quot;conceptual&quot; work such as the Kanjur, Tengyur, Nyingma Gyu Bum, Rinchen Terdzod, Nyingma Kama, Songs of Milarepa, and on and on.

Consider the Kanjur:

bdr:T2423 a Topic, Work ;
      rdfs:label &quot;bka&apos; &apos;gyur&quot;@bo-x-ewts ;
      :workHasTitle [ a :WorkTitle ;
            rdfs:label &quot;Kanjur&quot;@en ;
            :workHasTitleType bdr:TitleTypeBibliographicTitle ]

bdr:W9NEW01 a Work ;
      :workHasTitle [ a :WorkTitle ;
            rdfs:label &quot;Dege Kanjur&quot;@en ;
            :workHasTitleType bdr:TitleTypeBibliographicTitle ]
      :workExpressionOf bdr:T2423 .

bdr:W22703 a Work ;
      :workHasTitle [ a :WorkTitle ;
            rdfs:label &quot;Narthang Kanjur&quot;@en ;
            :workHasTitleType bdr:TitleTypeBibliographicTitle ]
      :workExpressionOf bdr:T2423 .

bdr:W26071 a Work ;
      :workHasTitle [ a :WorkTitle ;
            rdfs:label &quot;Lhasa Kanjur&quot;@en ;
            :workHasTitleType bdr:TitleTypeBibliographicTitle ]
      :workExpressionOf bdr:T2423 .</rdfs:comment>
        <rdfs:label xml:lang="en">expression of</rdfs:label>
    </owl:ObjectProperty>
    


    <!-- http://purl.bdrc.io/ontology/workGenre -->

    <owl:ObjectProperty rdf:about="http://purl.bdrc.io/ontology/workGenre">
        <rdfs:domain rdf:resource="http://purl.bdrc.io/ontology/Work"/>
        <rdfs:range rdf:resource="http://purl.bdrc.io/ontology/Topic"/>
        <rdfs:comment xml:lang="en">The referenced Topic is expected to be a &quot;genre&quot; topic and eventually the genre topics will be moved to a class of Genre and/or a Taxonomy of Genre may be supplied.

A genre is intended to capture a form or structural type of the work versus the content of the work.

For example, a composite :Work may have several genres and may be about several subjects:

bdr:W12827 a :Work ;
      :workHasGenre bdr:T132 ;
      :workHasGenre bdr:T1875 ;
      :workIsAbout bdr:T1388 ;
      :workIsAbout bdr:T317 ;
      :workIsAbout bdr:T354 ;

bdr:T132 a :Topic ;
      rdfs:label &quot;commentary&quot;@en .

bdr:T1875 a :Topic ;
      rdfs:label &quot;man ngag sde&quot;@bo-x-ewts .

bdr:T1388 a :Topic ;
      rdfs:label &quot;khregs chod&quot;@bo-x-ewts .

bdr:T317 a :Topic ;
      rdfs:label &quot;rdzogs chen sgrub mchod&quot;@bo-x-ewts .

bdr:T354 a :Topic ;
      rdfs:label &quot;rdzogs chen&quot;@bo-x-ewts .

This suggests that bdr:W12827 contains some commentaries and some instructions regarding dzogchen and so forth.</rdfs:comment>
        <rdfs:label xml:lang="en">has genre</rdfs:label>
    </owl:ObjectProperty>
    


    <!-- http://purl.bdrc.io/ontology/workHasDerivative -->

    <owl:ObjectProperty rdf:about="http://purl.bdrc.io/ontology/workHasDerivative">
        <rdfs:domain rdf:resource="http://purl.bdrc.io/ontology/Work"/>
        <rdfs:range rdf:resource="http://purl.bdrc.io/ontology/Work"/>
        <rdfs:comment xml:lang="en">The referenced work is a derivative of this work. This means that the referenced work may be a later edition or a version with some &quot;corrections&quot;/changes to the content of the referenced work.</rdfs:comment>
        <rdfs:label xml:lang="en">has derivative</rdfs:label>
        <rdfs:seeAlso rdf:resource="http://purl.bdrc.io/ontology/workDerivativeOf"/>
    </owl:ObjectProperty>
    


    <!-- http://purl.bdrc.io/ontology/workHasExpression -->

    <owl:ObjectProperty rdf:about="http://purl.bdrc.io/ontology/workHasExpression">
        <rdfs:domain rdf:resource="http://purl.bdrc.io/ontology/Work"/>
        <rdfs:range rdf:resource="http://purl.bdrc.io/ontology/Work"/>
        <rdfs:label xml:lang="en">has expression</rdfs:label>
        <rdfs:seeAlso rdf:resource="http://purl.bdrc.io/ontology/workExpressionOf"/>
    </owl:ObjectProperty>
    


    <!-- http://purl.bdrc.io/ontology/workHasHolding -->

    <owl:ObjectProperty rdf:about="http://purl.bdrc.io/ontology/workHasHolding">
        <rdfs:domain rdf:resource="http://purl.bdrc.io/ontology/Work"/>
        <rdfs:range rdf:resource="http://purl.bdrc.io/ontology/WorkHolding"/>
        <rdfs:comment xml:lang="en">References a :WorkHolding that describes a physical holding of this :Work at a particular Library (:Place).</rdfs:comment>
        <rdfs:label xml:lang="en">has holding</rdfs:label>
        <rdfs:seeAlso rdf:resource="http://purl.bdrc.io/ontology/WorkHolding"/>
    </owl:ObjectProperty>
    


    <!-- http://purl.bdrc.io/ontology/workHasItem -->

    <owl:ObjectProperty rdf:about="http://purl.bdrc.io/ontology/workHasItem">
        <rdfs:domain rdf:resource="http://purl.bdrc.io/ontology/Work"/>
        <rdfs:range rdf:resource="http://purl.bdrc.io/ontology/Item"/>
    </owl:ObjectProperty>
    


    <!-- http://purl.bdrc.io/ontology/workHasPart -->

    <owl:ObjectProperty rdf:about="http://purl.bdrc.io/ontology/workHasPart">
        <owl:inverseOf rdf:resource="http://purl.bdrc.io/ontology/workPartOf"/>
        <rdfs:domain rdf:resource="http://purl.bdrc.io/ontology/Work"/>
        <rdfs:range rdf:resource="http://purl.bdrc.io/ontology/Work"/>
        <rdfs:label xml:lang="en">has part</rdfs:label>
        <rdfs:seeAlso rdf:resource="http://purl.bdrc.io/ontology/workPartOf"/>
    </owl:ObjectProperty>
    


    <!-- http://purl.bdrc.io/ontology/workHasPubInfoSeries -->

    <owl:ObjectProperty rdf:about="http://purl.bdrc.io/ontology/workHasPubInfoSeries">
        <rdfs:domain rdf:resource="http://purl.bdrc.io/ontology/Work"/>
        <rdfs:range rdf:resource="http://purl.bdrc.io/ontology/WorkPubinfoSeries"/>
    </owl:ObjectProperty>
    


    <!-- http://purl.bdrc.io/ontology/workHasReproduction -->

    <owl:ObjectProperty rdf:about="http://purl.bdrc.io/ontology/workHasReproduction">
        <owl:inverseOf rdf:resource="http://purl.bdrc.io/ontology/workReproductionOf"/>
        <rdfs:domain rdf:resource="http://purl.bdrc.io/ontology/Work"/>
        <rdfs:range rdf:resource="http://purl.bdrc.io/ontology/Work"/>
        <rdfs:label xml:lang="en">has reproduction</rdfs:label>
        <rdfs:seeAlso rdf:resource="http://purl.bdrc.io/ontology/workReproductionOf"/>
    </owl:ObjectProperty>
    


    <!-- http://purl.bdrc.io/ontology/workHasSite -->

    <owl:ObjectProperty rdf:about="http://purl.bdrc.io/ontology/workHasSite">
        <rdfs:subPropertyOf rdf:resource="http://www.w3.org/2002/07/owl#topObjectProperty"/>
        <rdfs:domain rdf:resource="http://purl.bdrc.io/ontology/Work"/>
        <rdfs:range rdf:resource="http://purl.bdrc.io/ontology/WorkSite"/>
        <rdfs:comment xml:lang="en">A :WorkSite describes where some activity associated with a Work occurred. This was a component of the Outline nodes but has been folded into the general bibliographic model applicable to all :Work(s)</rdfs:comment>
        <rdfs:label xml:lang="en">has site</rdfs:label>
    </owl:ObjectProperty>
    


    <!-- http://purl.bdrc.io/ontology/workHasSourcePrintery -->

    <owl:ObjectProperty rdf:about="http://purl.bdrc.io/ontology/workHasSourcePrintery">
        <rdfs:domain rdf:resource="http://purl.bdrc.io/ontology/Work"/>
        <rdfs:range rdf:resource="http://purl.bdrc.io/ontology/Place"/>
    </owl:ObjectProperty>
    


    <!-- http://purl.bdrc.io/ontology/workHoldingLibrary -->

    <owl:ObjectProperty rdf:about="http://purl.bdrc.io/ontology/workHoldingLibrary">
        <rdfs:domain rdf:resource="http://purl.bdrc.io/ontology/WorkHolding"/>
        <rdfs:range rdf:resource="http://purl.bdrc.io/ontology/Place"/>
        <rdfs:comment xml:lang="en">The Library (Place) that contains the physical holding</rdfs:comment>
        <rdfs:label xml:lang="en">library</rdfs:label>
        <rdfs:seeAlso rdf:resource="http://purl.bdrc.io/ontology/WorkHolding"/>
    </owl:ObjectProperty>
    


    <!-- http://purl.bdrc.io/ontology/workInProduct -->

    <owl:ObjectProperty rdf:about="http://purl.bdrc.io/ontology/workInProduct">
        <rdfs:domain rdf:resource="http://purl.bdrc.io/ontology/Work"/>
        <rdfs:range rdf:resource="http://purl.bdrc.io/ontology/admin/Product"/>
    </owl:ObjectProperty>
    


    <!-- http://purl.bdrc.io/ontology/workIsAbout -->

    <owl:ObjectProperty rdf:about="http://purl.bdrc.io/ontology/workIsAbout">
        <rdfs:comment xml:lang="en">The referenced Entity is expected to be a subject of the work - something the work is about.

A composite :Work may have several genres and may be about several subjects:

bdr:W12827 a :Work ;
      :workHasGenre bdr:T132 ;
      :workHasGenre bdr:T1875 ;
      :workIsAbout bdr:T1388 ;
      :workIsAbout bdr:T317 ;
      :workIsAbout bdr:T354 ;

bdr:T132 a :Topic ;
      rdfs:label &quot;commentary&quot;@en .

bdr:T1875 a :Topic ;
      rdfs:label &quot;man ngag sde&quot;@bo-x-ewts .

bdr:T1388 a :Topic ;
      rdfs:label &quot;khregs chod&quot;@bo-x-ewts .

bdr:T317 a :Topic ;
      rdfs:label &quot;rdzogs chen sgrub mchod&quot;@bo-x-ewts .

bdr:T354 a :Topic ;
      rdfs:label &quot;rdzogs chen&quot;@bo-x-ewts .</rdfs:comment>
        <rdfs:label xml:lang="en">is about</rdfs:label>
    </owl:ObjectProperty>
    


    <!-- http://purl.bdrc.io/ontology/workIsSimilarTo -->

    <owl:ObjectProperty rdf:about="http://purl.bdrc.io/ontology/workIsSimilarTo">
        <rdf:type rdf:resource="http://www.w3.org/2002/07/owl#SymmetricProperty"/>
        <rdfs:domain rdf:resource="http://purl.bdrc.io/ontology/Work"/>
        <rdfs:range rdf:resource="http://purl.bdrc.io/ontology/Work"/>
        <rdfs:comment xml:lang="en">Indicates that two Works contents are similar to one another</rdfs:comment>
        <rdfs:label xml:lang="en">similar to</rdfs:label>
    </owl:ObjectProperty>
    


    <!-- http://purl.bdrc.io/ontology/workLocation -->

    <owl:ObjectProperty rdf:about="http://purl.bdrc.io/ontology/workLocation">
        <rdfs:domain rdf:resource="http://purl.bdrc.io/ontology/Lineage"/>
        <rdfs:range rdf:resource="http://purl.bdrc.io/ontology/WorkLocation"/>
        <rdfs:comment xml:lang="en">This is the location of the source information for this :Lineage in a specified gsan / thob yig.</rdfs:comment>
        <rdfs:comment xml:lang="en">the :workLocation may be used with other domains and these will be added in an owl:unionOf as they are added. One such is expected to be :Note</rdfs:comment>
        <rdfs:label xml:lang="en">source text</rdfs:label>
        <rdfs:seeAlso rdf:resource="http://purl.bdrc.io/ontology/Lineage"/>
    </owl:ObjectProperty>
    


    <!-- http://purl.bdrc.io/ontology/workLocationType -->

    <owl:ObjectProperty rdf:about="http://purl.bdrc.io/ontology/workLocationType">
        <rdfs:domain rdf:resource="http://purl.bdrc.io/ontology/WorkLocation"/>
        <rdfs:range rdf:resource="http://purl.bdrc.io/ontology/WorkLocationType"/>
        <rdfs:comment xml:lang="en">Indicates the type of the WorkLocation: beginning or end</rdfs:comment>
        <rdfs:comment xml:lang="en">location type</rdfs:comment>
    </owl:ObjectProperty>
    


    <!-- http://purl.bdrc.io/ontology/workLocationWork -->

    <owl:ObjectProperty rdf:about="http://purl.bdrc.io/ontology/workLocationWork">
        <rdfs:domain rdf:resource="http://purl.bdrc.io/ontology/WorkLocation"/>
        <rdfs:range rdf:resource="http://purl.bdrc.io/ontology/Work"/>
        <rdfs:label xml:lang="en">work location</rdfs:label>
        <rdfs:seeAlso rdf:resource="http://purl.bdrc.io/ontology/WorkLocation"/>
    </owl:ObjectProperty>
    


    <!-- http://purl.bdrc.io/ontology/workNumberOf -->

    <owl:ObjectProperty rdf:about="http://purl.bdrc.io/ontology/workNumberOf">
        <rdfs:domain rdf:resource="http://purl.bdrc.io/ontology/Work"/>
        <rdfs:range rdf:resource="http://purl.bdrc.io/ontology/Work"/>
        <rdfs:comment xml:lang="en">Indicates that this Work is a member of a series. This property is used rather than :workPartOf to distinguish between the situation in which a series is typically not published all at once versus a collection of Works such as a Kanjur or gSungbum that is conventionally published and distributed all at once.</rdfs:comment>
        <rdfs:comment xml:lang="en">Migration hint: Use this when a Work has &lt;w:info number=&quot;?&quot; parent=&quot;Wxxx&quot;/&gt; via:

bdr:Wwww :workNumberOf bdr:Wxxx .</rdfs:comment>
        <rdfs:label xml:lang="en">number of</rdfs:label>
    </owl:ObjectProperty>
    


    <!-- http://purl.bdrc.io/ontology/workPagination -->

    <owl:ObjectProperty rdf:about="http://purl.bdrc.io/ontology/workPagination">
        <rdfs:domain rdf:resource="http://purl.bdrc.io/ontology/WorkLocation"/>
        <rdfs:range rdf:resource="http://purl.bdrc.io/ontology/PaginationType"/>
        <rdfs:label xml:lang="en">pagination</rdfs:label>
        <rdfs:seeAlso rdf:resource="http://purl.bdrc.io/ontology/PaginationType"/>
    </owl:ObjectProperty>
    


    <!-- http://purl.bdrc.io/ontology/workPartOf -->

    <owl:ObjectProperty rdf:about="http://purl.bdrc.io/ontology/workPartOf">
        <rdfs:domain rdf:resource="http://purl.bdrc.io/ontology/Work"/>
        <rdfs:range rdf:resource="http://purl.bdrc.io/ontology/Work"/>
        <rdfs:comment xml:lang="en">The subject work is a part of the referenced work. The subject work in this case is an &lt;outline:node/&gt; in the legacy metadata. The referenced work may be the root work or another part of the root work such as a section.

For example, The Kanjur conventionally has a section of Vinaya texts and each of these will be a :Work modeled like:

bdr:SomeKanjurVinayaTextX a :Work ;
      :workPartOf bdr:SomeKanjurVinayaSection ;
      :workBeginsAt bdr:WorkLocationY001 ;
      :workEndsAt bdr:WorksLocationY002 .

bdr:SomeKanjurVinayaSection a :Work ;
      :workPartOf bdr:W26071 ;
      :workBeginsAt bdr:WorkLocationZ001 ;
      :workEndsAt bdr:WorksLocationZ002 .</rdfs:comment>
        <rdfs:label xml:lang="en">part of</rdfs:label>
    </owl:ObjectProperty>
    


    <!-- http://purl.bdrc.io/ontology/workPartType -->

    <owl:ObjectProperty rdf:about="http://purl.bdrc.io/ontology/workPartType">
        <rdfs:domain rdf:resource="http://purl.bdrc.io/ontology/Work"/>
        <rdfs:range rdf:resource="http://purl.bdrc.io/ontology/WorkPartType"/>
        <rdfs:comment xml:lang="en">If the subject Work :isPartOf another work then the referenced part type reflects the type of part: chapter, section, volume, etc</rdfs:comment>
        <rdfs:label xml:lang="en">part type</rdfs:label>
    </owl:ObjectProperty>
    


    <!-- http://purl.bdrc.io/ontology/workPrintType -->

    <owl:ObjectProperty rdf:about="http://purl.bdrc.io/ontology/workPrintType">
        <rdfs:domain rdf:resource="http://purl.bdrc.io/ontology/Work"/>
        <rdfs:range rdf:resource="http://purl.bdrc.io/ontology/PrintType"/>
    </owl:ObjectProperty>
    


    <!-- http://purl.bdrc.io/ontology/workReproductionOf -->

    <owl:ObjectProperty rdf:about="http://purl.bdrc.io/ontology/workReproductionOf">
        <rdfs:domain rdf:resource="http://purl.bdrc.io/ontology/Work"/>
        <rdfs:range rdf:resource="http://purl.bdrc.io/ontology/Work"/>
        <rdfs:comment xml:lang="en">The subject work is a reproduction of the referenced work such as a photocopy or a an offset print of an original or photocopy and so on. This is relevant to record versus :workExpressionOf when there may be features peculariar to the fact of reproduction versus a direct production such as from master woodblocks or, in a more modern setting, the original offset plates from an input text.

For example,

bdr:W22084 :workReproductionOf bdr:W9NEW01

indicates that bdr:W22084 is considered to be scanned images from a reproduction of the conceptual sdg dge Kanjur identified here as bdr:W9NEW01. The bdr:W9NEW01 denotes the constellation of versions/reproductions and derivatives of the (mythical) sde dge Kanjur.</rdfs:comment>
        <rdfs:label xml:lang="en">reproduction of</rdfs:label>
    </owl:ObjectProperty>
    


    <!-- http://purl.bdrc.io/ontology/workSitePlace -->

    <owl:ObjectProperty rdf:about="http://purl.bdrc.io/ontology/workSitePlace">
        <rdfs:subPropertyOf rdf:resource="http://www.w3.org/2002/07/owl#topObjectProperty"/>
        <rdfs:domain rdf:resource="http://purl.bdrc.io/ontology/WorkSite"/>
        <rdfs:range rdf:resource="http://purl.bdrc.io/ontology/Place"/>
        <rdfs:comment xml:lang="en">The place where some aspect of a Work occurred, such as the completion, editing, revelation and so on.</rdfs:comment>
        <rdfs:label xml:lang="en">work site place</rdfs:label>
    </owl:ObjectProperty>
    


    <!-- http://purl.bdrc.io/ontology/workSiteType -->

    <owl:ObjectProperty rdf:about="http://purl.bdrc.io/ontology/workSiteType">
        <rdfs:domain rdf:resource="http://purl.bdrc.io/ontology/WorkSite"/>
        <rdfs:range rdf:resource="http://purl.bdrc.io/ontology/WorkSiteType"/>
        <rdfs:comment xml:lang="en">The type of activity regarding a work that occurred at the indicated site. For example, the work was completed, edited, or started at the given site/place.</rdfs:comment>
        <rdfs:label xml:lang="en">work site type</rdfs:label>
    </owl:ObjectProperty>
    


    <!-- http://purl.bdrc.io/ontology/workTitle -->

    <owl:ObjectProperty rdf:about="http://purl.bdrc.io/ontology/workTitle">
        <rdfs:domain rdf:resource="http://purl.bdrc.io/ontology/Work"/>
        <rdfs:range rdf:resource="http://purl.bdrc.io/ontology/WorkTitle"/>
        <rdfs:comment xml:lang="en">Asserts that the subject Work has a particular title.</rdfs:comment>
        <rdfs:label xml:lang="en">has title</rdfs:label>
        <rdfs:seeAlso rdf:resource="http://purl.bdrc.io/ontology/WorkTitle"/>
    </owl:ObjectProperty>
    


    <!-- http://purl.bdrc.io/ontology/workTitleType -->

    <owl:ObjectProperty rdf:about="http://purl.bdrc.io/ontology/workTitleType">
        <rdfs:domain rdf:resource="http://purl.bdrc.io/ontology/WorkTitle"/>
        <rdfs:range rdf:resource="http://purl.bdrc.io/ontology/WorkTitleType"/>
        <rdfs:comment xml:lang="en">The type of the title, e.g., fullTitle, titlePageTitle and so on</rdfs:comment>
        <rdfs:label xml:lang="en">type</rdfs:label>
        <rdfs:seeAlso rdf:resource="http://purl.bdrc.io/ontology/WorkTitle"/>
    </owl:ObjectProperty>
    


    <!-- http://purl.bdrc.io/ontology/workTranslationOf -->

    <owl:ObjectProperty rdf:about="http://purl.bdrc.io/ontology/workTranslationOf">
        <owl:inverseOf rdf:resource="http://purl.bdrc.io/ontology/workhasTranslation"/>
        <rdfs:domain rdf:resource="http://purl.bdrc.io/ontology/Work"/>
        <rdfs:range rdf:resource="http://purl.bdrc.io/ontology/Work"/>
        <rdfs:comment xml:lang="en">The subject work is identified as a translation of the referenced work. This will be used, for example, when the subject work is a Tibetan translation of a referenced Sanskrit work.</rdfs:comment>
        <rdfs:label xml:lang="en">translation of</rdfs:label>
    </owl:ObjectProperty>
    


    <!-- http://purl.bdrc.io/ontology/workType -->

    <owl:ObjectProperty rdf:about="http://purl.bdrc.io/ontology/workType">
        <rdfs:domain rdf:resource="http://purl.bdrc.io/ontology/Work"/>
        <rdfs:range rdf:resource="http://purl.bdrc.io/ontology/WorkType"/>
        <rdfs:comment xml:lang="en">Migration info: This is the &lt;work:info @nodeType/&gt; attribute NOT the unused @type attribute</rdfs:comment>
        <rdfs:label xml:lang="en">has type</rdfs:label>
        <rdfs:seeAlso rdf:resource="http://purl.bdrc.io/ontology/WorkType"/>
    </owl:ObjectProperty>
    


    <!-- http://purl.bdrc.io/ontology/workhasTranslation -->

    <owl:ObjectProperty rdf:about="http://purl.bdrc.io/ontology/workhasTranslation">
        <rdfs:domain rdf:resource="http://purl.bdrc.io/ontology/Work"/>
        <rdfs:range rdf:resource="http://purl.bdrc.io/ontology/Work"/>
        <rdfs:comment xml:lang="en">The referenced work is identified as a translation of the subject work. This will be used, for example, when the referenced work is a Tibetan translation of a subject Sanskrit work.</rdfs:comment>
        <rdfs:label xml:lang="en">has translation</rdfs:label>
    </owl:ObjectProperty>
    


    <!-- http://purl.bdrc.io/ontology/admin/productHasOrg -->

    <owl:ObjectProperty rdf:about="http://purl.bdrc.io/ontology/admin/productHasOrg">
        <rdfs:domain>
            <owl:Class>
                <owl:unionOf rdf:parseType="Collection">
                    <rdf:Description rdf:about="http://purl.bdrc.io/ontology/admin/Product"/>
                    <rdf:Description rdf:about="http://purl.bdrc.io/ontology/admin/ProductOrg"/>
                </owl:unionOf>
            </owl:Class>
        </rdfs:domain>
        <rdfs:range rdf:resource="http://purl.bdrc.io/ontology/admin/ProductOrg"/>
        <rdfs:comment xml:lang="en">Allows to compose an organization in terms of sub-organizations. Useful for large organizations such as University of California system for which there are many address ranges for each campus such as UC Berkeley and UCLA and so on</rdfs:comment>
    </owl:ObjectProperty>
    


    <!-- 
    ///////////////////////////////////////////////////////////////////////////////////////
    //
    // Data properties
    //
    ///////////////////////////////////////////////////////////////////////////////////////
     -->

    


    <!-- http://purl.bdrc.io/ontology/addressCity -->

    <owl:DatatypeProperty rdf:about="http://purl.bdrc.io/ontology/addressCity">
        <rdfs:domain rdf:resource="http://purl.bdrc.io/ontology/PlaceAddress"/>
        <rdfs:range rdf:resource="http://www.w3.org/2001/XMLSchema#string"/>
        <rdfs:label xml:lang="en">city</rdfs:label>
    </owl:DatatypeProperty>
    


    <!-- http://purl.bdrc.io/ontology/addressCountry -->

    <owl:DatatypeProperty rdf:about="http://purl.bdrc.io/ontology/addressCountry">
        <rdfs:domain rdf:resource="http://purl.bdrc.io/ontology/PlaceAddress"/>
        <rdfs:range rdf:resource="http://www.w3.org/2001/XMLSchema#string"/>
        <rdfs:label xml:lang="en">country</rdfs:label>
    </owl:DatatypeProperty>
    


    <!-- http://purl.bdrc.io/ontology/addressNumber -->

    <owl:DatatypeProperty rdf:about="http://purl.bdrc.io/ontology/addressNumber">
        <rdfs:domain rdf:resource="http://purl.bdrc.io/ontology/PlaceAddress"/>
        <rdfs:range rdf:resource="http://www.w3.org/2001/XMLSchema#string"/>
        <rdfs:label xml:lang="en">number</rdfs:label>
    </owl:DatatypeProperty>
    


    <!-- http://purl.bdrc.io/ontology/addressPostal -->

    <owl:DatatypeProperty rdf:about="http://purl.bdrc.io/ontology/addressPostal">
        <rdfs:domain rdf:resource="http://purl.bdrc.io/ontology/PlaceAddress"/>
        <rdfs:range rdf:resource="http://www.w3.org/2001/XMLSchema#string"/>
        <rdfs:label xml:lang="en">postasl code</rdfs:label>
    </owl:DatatypeProperty>
    


    <!-- http://purl.bdrc.io/ontology/addressState -->

    <owl:DatatypeProperty rdf:about="http://purl.bdrc.io/ontology/addressState">
        <rdfs:domain rdf:resource="http://purl.bdrc.io/ontology/PlaceAddress"/>
        <rdfs:range rdf:resource="http://www.w3.org/2001/XMLSchema#string"/>
        <rdfs:label xml:lang="en">state</rdfs:label>
    </owl:DatatypeProperty>
    


    <!-- http://purl.bdrc.io/ontology/addressStreet -->

    <owl:DatatypeProperty rdf:about="http://purl.bdrc.io/ontology/addressStreet">
        <rdfs:domain rdf:resource="http://purl.bdrc.io/ontology/PlaceAddress"/>
        <rdfs:range rdf:resource="http://www.w3.org/2001/XMLSchema#string"/>
        <rdfs:label xml:lang="en">street</rdfs:label>
    </owl:DatatypeProperty>
    


    <!-- http://purl.bdrc.io/ontology/desc_NoType -->

    <owl:DatatypeProperty rdf:about="http://purl.bdrc.io/ontology/desc_NoType">
        <rdfs:range rdf:resource="http://www.w3.org/2001/XMLSchema#string"/>
        <rdfs:label xml:lang="en">description with no type</rdfs:label>
    </owl:DatatypeProperty>
    


    <!-- http://purl.bdrc.io/ontology/description -->

    <owl:DatatypeProperty rdf:about="http://purl.bdrc.io/ontology/description">
        <rdfs:range rdf:resource="http://www.w3.org/1999/02/22-rdf-syntax-ns#PlainLiteral"/>
    </owl:DatatypeProperty>
    


    <!-- http://purl.bdrc.io/ontology/external_content -->

    <owl:DatatypeProperty rdf:about="http://purl.bdrc.io/ontology/external_content">
        <rdfs:subPropertyOf rdf:resource="http://www.w3.org/2002/07/owl#topDataProperty"/>
        <rdfs:domain rdf:resource="http://purl.bdrc.io/ontology/External"/>
        <rdfs:range rdf:resource="http://www.w3.org/1999/02/22-rdf-syntax-ns#PlainLiteral"/>
    </owl:DatatypeProperty>
    


    <!-- http://purl.bdrc.io/ontology/external_data -->

    <owl:DatatypeProperty rdf:about="http://purl.bdrc.io/ontology/external_data">
        <rdfs:subPropertyOf rdf:resource="http://www.w3.org/2002/07/owl#topDataProperty"/>
        <rdfs:domain rdf:resource="http://purl.bdrc.io/ontology/External"/>
        <rdfs:range rdf:resource="http://www.w3.org/2001/XMLSchema#anyURI"/>
        <rdfs:comment>this should be the link to the specific item that is related to this Work, Person, Place and so on.</rdfs:comment>
    </owl:DatatypeProperty>
    


    <!-- http://purl.bdrc.io/ontology/external_source -->

    <owl:DatatypeProperty rdf:about="http://purl.bdrc.io/ontology/external_source">
        <rdfs:subPropertyOf rdf:resource="http://www.w3.org/2002/07/owl#topDataProperty"/>
        <rdfs:domain rdf:resource="http://purl.bdrc.io/ontology/External"/>
        <rdfs:range rdf:resource="http://www.w3.org/2001/XMLSchema#anyURI"/>
        <rdfs:comment>a link to the top-level of an external resource such as a http://treasuryoflives.org.</rdfs:comment>
    </owl:DatatypeProperty>
    


    <!-- http://purl.bdrc.io/ontology/itemBDRCHoldingStatement -->

    <owl:DatatypeProperty rdf:about="http://purl.bdrc.io/ontology/itemBDRCHoldingStatement">
        <rdfs:domain rdf:resource="http://purl.bdrc.io/ontology/Item"/>
        <rdfs:range rdf:resource="http://www.w3.org/2001/XMLSchema#string"/>
        <rdfs:comment xml:lang="en">A free-text statement of the holdings by BDRC of this Item (and its relatives).</rdfs:comment>
        <rdfs:comment xml:lang="en">Migration hint: the &lt;pubinfo:tbrcHoldings/&gt; should be mapped to :itemBDRCHoldingStatement on the associated Item.

This might require creating an otherwise empty Item to stand-in for a Work that has yet to be scanned.</rdfs:comment>
        <rdfs:label xml:lang="en">BDRC holdings statement</rdfs:label>
    </owl:DatatypeProperty>
    


    <!-- http://purl.bdrc.io/ontology/name -->

    <owl:DatatypeProperty rdf:about="http://purl.bdrc.io/ontology/name">
        <rdfs:range rdf:resource="http://www.w3.org/1999/02/22-rdf-syntax-ns#PlainLiteral"/>
        <rdfs:comment xml:lang="en">whenever a name (or title) is needed such as for Place, Office, PersonName and so on. Use of the rdfs:label is reserved for &quot;primary&quot; display purposes, i.e., the name (or title) that is used when identifying the resource on a web page or the like.</rdfs:comment>
        <rdfs:label xml:lang="en">name</rdfs:label>
    </owl:DatatypeProperty>
    


    <!-- http://purl.bdrc.io/ontology/onOrAbout -->

    <owl:DatatypeProperty rdf:about="http://purl.bdrc.io/ontology/onOrAbout">
        <rdfs:range rdf:resource="http://www.w3.org/2001/XMLSchema#string"/>
        <rdfs:comment xml:lang="en">This property replaces the various separate circa properties with a single property that will have a single validator and editor support.</rdfs:comment>
        <rdfs:label xml:lang="en">circa</rdfs:label>
    </owl:DatatypeProperty>
    


    <!-- http://purl.bdrc.io/ontology/personIsNonActor -->

    <owl:DatatypeProperty rdf:about="http://purl.bdrc.io/ontology/personIsNonActor">
        <rdfs:subPropertyOf rdf:resource="http://www.w3.org/2002/07/owl#topDataProperty"/>
        <rdfs:domain rdf:resource="http://purl.bdrc.io/ontology/Person"/>
        <rdfs:range rdf:resource="http://www.w3.org/2001/XMLSchema#boolean"/>
        <rdfs:comment xml:lang="en">The source person.xsd includes @type on &lt;info/&gt; which is meant to capture whether the Person is an &quot;actor&quot; in the world of Tibetan books. There are 40 out of 18,320 individuals that have been marked as info/@type = nonActor. These 40 are non-Tibetan individuals that have been included in the db because they are translators, or authors of some work of interest. Many of the records of nonActors have various small errors that need to be corrected.

In any event, when a per:Person is being migrated with info/@type = nonactor then simply assert:  p? :personNonActor true, and we will be able to locate these individuals after migration for further attention</rdfs:comment>
        <rdfs:label xml:lang="en">non actor</rdfs:label>
    </owl:DatatypeProperty>
    


    <!-- http://purl.bdrc.io/ontology/placeAccuracy -->

    <owl:DatatypeProperty rdf:about="http://purl.bdrc.io/ontology/placeAccuracy">
        <rdfs:domain rdf:resource="http://purl.bdrc.io/ontology/Place"/>
        <rdfs:range rdf:resource="http://www.w3.org/2001/XMLSchema#string"/>
        <rdfs:comment xml:lang="en">The accuracy of the latitude and longitude</rdfs:comment>
        <rdfs:label xml:lang="en">accuracy</rdfs:label>
    </owl:DatatypeProperty>
    


    <!-- http://purl.bdrc.io/ontology/placeChgisId -->

    <owl:DatatypeProperty rdf:about="http://purl.bdrc.io/ontology/placeChgisId">
        <rdfs:domain rdf:resource="http://purl.bdrc.io/ontology/Place"/>
        <rdfs:range rdf:resource="http://www.w3.org/2001/XMLSchema#string"/>
        <rdfs:comment xml:lang="en">A legacy Chinese gis id for the Place provided during migration of historical Tibetan Places by Karl Ryavec and Lex Berman</rdfs:comment>
        <rdfs:comment xml:lang="en">chgis id</rdfs:comment>
    </owl:DatatypeProperty>
    


    <!-- http://purl.bdrc.io/ontology/placeGB2260-2013 -->

    <owl:DatatypeProperty rdf:about="http://purl.bdrc.io/ontology/placeGB2260-2013">
        <rdfs:domain rdf:resource="http://purl.bdrc.io/ontology/Place"/>
        <rdfs:range rdf:resource="http://www.w3.org/2001/XMLSchema#string"/>
        <rdfs:comment xml:lang="en">The 2013 Chinese GB code for the Place. Similar to U.S. Zipcode</rdfs:comment>
        <rdfs:label xml:lang="en">GB2260-2013</rdfs:label>
    </owl:DatatypeProperty>
    


    <!-- http://purl.bdrc.io/ontology/placeGonpaPerEcumen -->

    <owl:DatatypeProperty rdf:about="http://purl.bdrc.io/ontology/placeGonpaPerEcumen">
        <rdfs:domain rdf:resource="http://purl.bdrc.io/ontology/Place"/>
        <rdfs:range rdf:resource="http://www.w3.org/2001/XMLSchema#string"/>
        <rdfs:comment xml:lang="en">Karl Ryavec supplies the following information regarding this property:

Gonpa per ecumen would be how many temples are there per one sq km of land area minus water, bare rock, ice and so forth.  Thus I totaled the ecumen areas of each township primarily in terms of the sq km of grassland and forests and farmland.  Then because these areas per temple are so tiny I represented the final amounts on my map legend per 1000 sq km so that the numbers would be closer to 1.0 at times.  For example there might only be .0000001 temples per sq km of ecumen.  But if we convert to per 1000 sq km of ecumen we get .0001 temples  which is a more understandable amount.  Though I think most scholars are baffled by technology and so just understand the idea of core areas like the Lhasa valley compared the peripheral areas like the Changthang.  So that&apos;s mainly what I focused on showing.</rdfs:comment>
        <rdfs:comment xml:lang="en">The number of monasteries per ecumen in this Place (presumably a region) from data provided by Karl Ryavec</rdfs:comment>
        <rdfs:label xml:lang="en">monasteries per ecumen</rdfs:label>
    </owl:DatatypeProperty>
    


    <!-- http://purl.bdrc.io/ontology/placeLat -->

    <owl:DatatypeProperty rdf:about="http://purl.bdrc.io/ontology/placeLat">
        <rdf:type rdf:resource="http://www.w3.org/2002/07/owl#FunctionalProperty"/>
        <rdfs:domain rdf:resource="http://purl.bdrc.io/ontology/Place"/>
        <rdfs:range rdf:resource="http://www.w3.org/2001/XMLSchema#string"/>
        <rdfs:comment xml:lang="en">The latitude of the Place</rdfs:comment>
        <rdfs:label xml:lang="en">latitude</rdfs:label>
    </owl:DatatypeProperty>
    


    <!-- http://purl.bdrc.io/ontology/placeLong -->

    <owl:DatatypeProperty rdf:about="http://purl.bdrc.io/ontology/placeLong">
        <rdf:type rdf:resource="http://www.w3.org/2002/07/owl#FunctionalProperty"/>
        <rdfs:domain rdf:resource="http://purl.bdrc.io/ontology/Place"/>
        <rdfs:range rdf:resource="http://www.w3.org/2001/XMLSchema#string"/>
        <rdfs:comment xml:lang="en">The longitude of the Place</rdfs:comment>
        <rdfs:label xml:lang="en">longitude</rdfs:label>
    </owl:DatatypeProperty>
    


    <!-- http://purl.bdrc.io/ontology/placeRegionPoly -->

    <owl:DatatypeProperty rdf:about="http://purl.bdrc.io/ontology/placeRegionPoly">
        <rdfs:domain rdf:resource="http://purl.bdrc.io/ontology/Place"/>
        <rdfs:range rdf:resource="http://www.w3.org/2001/XMLSchema#string"/>
        <rdfs:comment>The object of this property is an xsd:string representing a geoJSON Polygon or Mulit-Polygon. See http://geojson.org/geojson-spec.html</rdfs:comment>
        <rdfs:label xml:lang="en">region poly</rdfs:label>
    </owl:DatatypeProperty>
    


    <!-- http://purl.bdrc.io/ontology/placeWB2000 -->

    <owl:DatatypeProperty rdf:about="http://purl.bdrc.io/ontology/placeWB2000">
        <rdf:type rdf:resource="http://www.w3.org/2002/07/owl#FunctionalProperty"/>
        <rdfs:domain rdf:resource="http://purl.bdrc.io/ontology/Place"/>
        <rdfs:range rdf:resource="http://www.w3.org/2001/XMLSchema#integer"/>
        <rdfs:comment xml:lang="en">THe World Bank 2000 population for the Place</rdfs:comment>
    </owl:DatatypeProperty>
    


    <!-- http://purl.bdrc.io/ontology/placeWB2010 -->

    <owl:DatatypeProperty rdf:about="http://purl.bdrc.io/ontology/placeWB2010">
        <rdf:type rdf:resource="http://www.w3.org/2002/07/owl#FunctionalProperty"/>
        <rdfs:domain rdf:resource="http://purl.bdrc.io/ontology/Place"/>
        <rdfs:range rdf:resource="http://www.w3.org/2001/XMLSchema#integer"/>
        <rdfs:comment xml:lang="en">The World Bank 2010 population for the Place</rdfs:comment>
        <rdfs:label xml:lang="en">WB 2010 population</rdfs:label>
    </owl:DatatypeProperty>
    


    <!-- http://purl.bdrc.io/ontology/placeWBArea -->

    <owl:DatatypeProperty rdf:about="http://purl.bdrc.io/ontology/placeWBArea">
        <rdfs:domain rdf:resource="http://purl.bdrc.io/ontology/Place"/>
        <rdfs:range rdf:resource="http://www.w3.org/2001/XMLSchema#integer"/>
        <rdfs:comment xml:lang="en">The area in square km of the Place from the World Bank 2010</rdfs:comment>
    </owl:DatatypeProperty>
    


    <!-- http://purl.bdrc.io/ontology/volumeImageList -->

    <owl:DatatypeProperty rdf:about="http://purl.bdrc.io/ontology/volumeImageList">
        <rdfs:domain rdf:resource="http://purl.bdrc.io/ontology/Volume"/>
        <rdfs:range rdf:resource="http://www.w3.org/2001/XMLSchema#string"/>
        <rdfs:comment>this property appears as &lt;ig:description type=&quot;onDisk&quot;/&gt; in the source documents</rdfs:comment>
    </owl:DatatypeProperty>
    


    <!-- http://purl.bdrc.io/ontology/volumeNumber -->

    <owl:DatatypeProperty rdf:about="http://purl.bdrc.io/ontology/volumeNumber">
        <rdfs:domain rdf:resource="http://purl.bdrc.io/ontology/Volume"/>
        <rdfs:range>
            <rdfs:Datatype>
                <owl:unionOf rdf:parseType="Collection">
                    <rdf:Description rdf:about="http://www.w3.org/2001/XMLSchema#positiveInteger"/>
                    <rdf:Description rdf:about="http://www.w3.org/2001/XMLSchema#string"/>
                </owl:unionOf>
            </rdfs:Datatype>
        </rdfs:range>
    </owl:DatatypeProperty>
    


    <!-- http://purl.bdrc.io/ontology/volumePagesIntro -->

    <owl:DatatypeProperty rdf:about="http://purl.bdrc.io/ontology/volumePagesIntro">
        <rdfs:domain rdf:resource="http://purl.bdrc.io/ontology/Volume"/>
        <rdfs:range rdf:resource="http://www.w3.org/2001/XMLSchema#nonNegativeInteger"/>
    </owl:DatatypeProperty>
    


    <!-- http://purl.bdrc.io/ontology/volumePagesTbrcIntro -->

    <owl:DatatypeProperty rdf:about="http://purl.bdrc.io/ontology/volumePagesTbrcIntro">
        <rdfs:domain rdf:resource="http://purl.bdrc.io/ontology/Volume"/>
        <rdfs:range rdf:resource="http://www.w3.org/2001/XMLSchema#nonNegativeInteger"/>
    </owl:DatatypeProperty>
    


    <!-- http://purl.bdrc.io/ontology/volumePagesText -->

    <owl:DatatypeProperty rdf:about="http://purl.bdrc.io/ontology/volumePagesText">
        <rdfs:domain rdf:resource="http://purl.bdrc.io/ontology/Volume"/>
        <rdfs:range rdf:resource="http://www.w3.org/2001/XMLSchema#nonNegativeInteger"/>
    </owl:DatatypeProperty>
    


    <!-- http://purl.bdrc.io/ontology/volumePagesTotal -->

    <owl:DatatypeProperty rdf:about="http://purl.bdrc.io/ontology/volumePagesTotal">
        <rdfs:domain rdf:resource="http://purl.bdrc.io/ontology/Volume"/>
        <rdfs:range rdf:resource="http://www.w3.org/2001/XMLSchema#positiveInteger"/>
    </owl:DatatypeProperty>
    


    <!-- http://purl.bdrc.io/ontology/workAuthorshipStatement -->

    <owl:DatatypeProperty rdf:about="http://purl.bdrc.io/ontology/workAuthorshipStatement">
        <rdfs:domain rdf:resource="http://purl.bdrc.io/ontology/Work"/>
        <rdfs:range rdf:resource="http://www.w3.org/1999/02/22-rdf-syntax-ns#PlainLiteral"/>
        <rdfs:comment xml:lang="en">Authorship statement for the Work.</rdfs:comment>
        <rdfs:comment xml:lang="en">Migration hint: Use this when migrating &lt;o:description type=&quot;authorship&quot;/&gt;</rdfs:comment>
        <rdfs:label xml:lang="en">authorship</rdfs:label>
    </owl:DatatypeProperty>
    


    <!-- http://purl.bdrc.io/ontology/workBiblioNote -->

    <owl:DatatypeProperty rdf:about="http://purl.bdrc.io/ontology/workBiblioNote">
        <rdfs:domain rdf:resource="http://purl.bdrc.io/ontology/Work"/>
        <rdfs:range rdf:resource="http://www.w3.org/1999/02/22-rdf-syntax-ns#PlainLiteral"/>
    </owl:DatatypeProperty>
    


    <!-- http://purl.bdrc.io/ontology/workBiblioStatus -->

    <owl:DatatypeProperty rdf:about="http://purl.bdrc.io/ontology/workBiblioStatus">
        <rdfs:domain rdf:resource="http://purl.bdrc.io/ontology/Work"/>
        <rdfs:range rdf:resource="http://www.w3.org/1999/02/22-rdf-syntax-ns#PlainLiteral"/>
        <rdfs:comment xml:lang="en">A bibliogrpahic status statement in the language of the Work</rdfs:comment>
        <rdfs:comment xml:lang="en">Migration hint: this is used for &lt;o:description type=&quot;status&quot;/&gt;</rdfs:comment>
        <rdfs:label xml:lang="en">bibliographic status statement</rdfs:label>
    </owl:DatatypeProperty>
    


    <!-- http://purl.bdrc.io/ontology/workCatalogInfo -->

    <owl:DatatypeProperty rdf:about="http://purl.bdrc.io/ontology/workCatalogInfo">
        <rdfs:domain rdf:resource="http://purl.bdrc.io/ontology/Work"/>
        <rdfs:range rdf:resource="http://www.w3.org/1999/02/22-rdf-syntax-ns#PlainLiteral"/>
    </owl:DatatypeProperty>
    


    <!-- http://purl.bdrc.io/ontology/workColophon -->

    <owl:DatatypeProperty rdf:about="http://purl.bdrc.io/ontology/workColophon">
        <rdfs:domain rdf:resource="http://purl.bdrc.io/ontology/Work"/>
        <rdfs:range rdf:resource="http://www.w3.org/1999/02/22-rdf-syntax-ns#PlainLiteral"/>
        <rdfs:comment xml:lang="en">This was the description of type colophon which was used primarily (exclusively?) on &lt;outline:node/&gt;s. It is now part of the extended bibliographic model allowing to tag any sort of Work with a colophon</rdfs:comment>
        <rdfs:label xml:lang="en">colophon</rdfs:label>
    </owl:DatatypeProperty>
    


    <!-- http://purl.bdrc.io/ontology/workCompletionDate -->

    <owl:DatatypeProperty rdf:about="http://purl.bdrc.io/ontology/workCompletionDate">
        <rdfs:domain rdf:resource="http://purl.bdrc.io/ontology/Work"/>
        <rdfs:range rdf:resource="http://www.w3.org/2001/XMLSchema#string"/>
        <rdfs:comment xml:lang="en">Migration hint: from &lt;o:description type=&quot;completionDate&quot;/&gt;</rdfs:comment>
        <rdfs:comment xml:lang="en">Records the declared date of completion for the Work - typically from the colophon</rdfs:comment>
        <rdfs:label xml:lang="en">completion date</rdfs:label>
    </owl:DatatypeProperty>
    


    <!-- http://purl.bdrc.io/ontology/workContainsChapters -->

    <owl:DatatypeProperty rdf:about="http://purl.bdrc.io/ontology/workContainsChapters">
        <rdfs:domain rdf:resource="http://purl.bdrc.io/ontology/Work"/>
        <rdfs:range rdf:resource="http://www.w3.org/2001/XMLSchema#string"/>
        <rdfs:comment xml:lang="en">Migration hint: &lt;o:description type=&quot;chapters&quot;/&gt;</rdfs:comment>
        <rdfs:comment xml:lang="en">records the chapters of a larger Work contained in this Work</rdfs:comment>
        <rdfs:label xml:lang="en">chapters contained</rdfs:label>
    </owl:DatatypeProperty>
    


    <!-- http://purl.bdrc.io/ontology/workDateOfWriting -->

    <owl:DatatypeProperty rdf:about="http://purl.bdrc.io/ontology/workDateOfWriting">
        <rdfs:domain rdf:resource="http://purl.bdrc.io/ontology/Work"/>
        <rdfs:range rdf:resource="http://www.w3.org/2001/XMLSchema#string"/>
    </owl:DatatypeProperty>
    


    <!-- http://purl.bdrc.io/ontology/workDimensions -->

    <owl:DatatypeProperty rdf:about="http://purl.bdrc.io/ontology/workDimensions">
        <rdfs:domain rdf:resource="http://purl.bdrc.io/ontology/Work"/>
        <rdfs:range rdf:resource="http://www.w3.org/2001/XMLSchema#string"/>
    </owl:DatatypeProperty>
    


    <!-- http://purl.bdrc.io/ontology/workEditionStatement -->

    <owl:DatatypeProperty rdf:about="http://purl.bdrc.io/ontology/workEditionStatement">
        <rdfs:domain rdf:resource="http://purl.bdrc.io/ontology/Work"/>
        <rdfs:range rdf:resource="http://www.w3.org/1999/02/22-rdf-syntax-ns#PlainLiteral"/>
    </owl:DatatypeProperty>
    


    <!-- http://purl.bdrc.io/ontology/workEncoding -->

    <owl:DatatypeProperty rdf:about="http://purl.bdrc.io/ontology/workEncoding">
        <rdfs:domain rdf:resource="http://purl.bdrc.io/ontology/Work"/>
        <rdfs:range rdf:resource="http://www.w3.org/2001/XMLSchema#string"/>
    </owl:DatatypeProperty>
    


    <!-- http://purl.bdrc.io/ontology/workErrata -->

    <owl:DatatypeProperty rdf:about="http://purl.bdrc.io/ontology/workErrata">
        <rdfs:domain rdf:resource="http://purl.bdrc.io/ontology/Work"/>
        <rdfs:range rdf:resource="http://www.w3.org/1999/02/22-rdf-syntax-ns#PlainLiteral"/>
        <rdfs:comment xml:lang="en">Indicates a statement of error in the content</rdfs:comment>
        <rdfs:label xml:lang="en">errata</rdfs:label>
    </owl:DatatypeProperty>
    


    <!-- http://purl.bdrc.io/ontology/workExtentStatement -->

    <owl:DatatypeProperty rdf:about="http://purl.bdrc.io/ontology/workExtentStatement">
        <rdfs:domain rdf:resource="http://purl.bdrc.io/ontology/Work"/>
        <rdfs:range rdf:resource="http://www.w3.org/2001/XMLSchema#string"/>
        <rdfs:comment xml:lang="en">A statement of the extent of the Work</rdfs:comment>
        <rdfs:comment xml:lang="en">Migration hint: use also for &lt;o:description type=&quot;extent&quot;/&gt;</rdfs:comment>
        <rdfs:label xml:lang="en">extent statement</rdfs:label>
    </owl:DatatypeProperty>
    


    <!-- http://purl.bdrc.io/ontology/workHoldingCode -->

    <owl:DatatypeProperty rdf:about="http://purl.bdrc.io/ontology/workHoldingCode">
        <rdfs:domain rdf:resource="http://purl.bdrc.io/ontology/WorkHolding"/>
        <rdfs:range rdf:resource="http://www.w3.org/2001/XMLSchema#string"/>
        <rdfs:comment xml:lang="en">Code indicating the library</rdfs:comment>
        <rdfs:label xml:lang="en">code</rdfs:label>
        <rdfs:seeAlso rdf:resource="http://purl.bdrc.io/ontology/WorkHolding"/>
    </owl:DatatypeProperty>
    


    <!-- http://purl.bdrc.io/ontology/workHoldingCopies -->

    <owl:DatatypeProperty rdf:about="http://purl.bdrc.io/ontology/workHoldingCopies">
        <rdfs:domain rdf:resource="http://purl.bdrc.io/ontology/WorkHolding"/>
        <rdfs:range rdf:resource="http://www.w3.org/2001/XMLSchema#string"/>
        <rdfs:comment xml:lang="en">The number of copies of the :Work in this holding</rdfs:comment>
        <rdfs:label xml:lang="en">copies</rdfs:label>
        <rdfs:seeAlso rdf:resource="http://purl.bdrc.io/ontology/WorkHolding"/>
    </owl:DatatypeProperty>
    


    <!-- http://purl.bdrc.io/ontology/workHoldingException -->

    <owl:DatatypeProperty rdf:about="http://purl.bdrc.io/ontology/workHoldingException">
        <rdfs:domain rdf:resource="http://purl.bdrc.io/ontology/WorkHolding"/>
        <rdfs:range rdf:resource="http://www.w3.org/1999/02/22-rdf-syntax-ns#PlainLiteral"/>
        <rdfs:comment xml:lang="en">Exception notes such a missing volume, damage to pages and so on</rdfs:comment>
        <rdfs:label xml:lang="en">exception</rdfs:label>
        <rdfs:seeAlso rdf:resource="http://purl.bdrc.io/ontology/WorkHolding"/>
    </owl:DatatypeProperty>
    


    <!-- http://purl.bdrc.io/ontology/workHoldingShelf -->

    <owl:DatatypeProperty rdf:about="http://purl.bdrc.io/ontology/workHoldingShelf">
        <rdfs:domain rdf:resource="http://purl.bdrc.io/ontology/WorkHolding"/>
        <rdfs:range rdf:resource="http://www.w3.org/2001/XMLSchema#string"/>
        <rdfs:comment xml:lang="en">Identifies where the holding is shelved. The shelf code is based on a library specific taxonomy</rdfs:comment>
        <rdfs:label xml:lang="en">shelf</rdfs:label>
        <rdfs:seeAlso rdf:resource="http://purl.bdrc.io/ontology/WorkHolding"/>
    </owl:DatatypeProperty>
    


    <!-- http://purl.bdrc.io/ontology/workHollis -->

    <owl:DatatypeProperty rdf:about="http://purl.bdrc.io/ontology/workHollis">
        <rdfs:domain rdf:resource="http://purl.bdrc.io/ontology/Work"/>
        <rdfs:range rdf:resource="http://www.w3.org/2001/XMLSchema#string"/>
    </owl:DatatypeProperty>
    


    <!-- http://purl.bdrc.io/ontology/workIllustrations -->

    <owl:DatatypeProperty rdf:about="http://purl.bdrc.io/ontology/workIllustrations">
        <rdfs:domain rdf:resource="http://purl.bdrc.io/ontology/Work"/>
        <rdfs:range rdf:resource="http://www.w3.org/2001/XMLSchema#string"/>
    </owl:DatatypeProperty>
    


    <!-- http://purl.bdrc.io/ontology/workIncipit -->

    <owl:DatatypeProperty rdf:about="http://purl.bdrc.io/ontology/workIncipit">
        <rdfs:domain rdf:resource="http://purl.bdrc.io/ontology/Work"/>
        <rdfs:range rdf:resource="http://www.w3.org/1999/02/22-rdf-syntax-ns#PlainLiteral"/>
        <rdfs:comment xml:lang="en">The opening words of the Work</rdfs:comment>
        <rdfs:label xml:lang="en">incipit</rdfs:label>
    </owl:DatatypeProperty>
    


    <!-- http://purl.bdrc.io/ontology/workIsNumbered -->

    <owl:DatatypeProperty rdf:about="http://purl.bdrc.io/ontology/workIsNumbered">
        <rdfs:domain rdf:resource="http://purl.bdrc.io/ontology/Work"/>
        <rdfs:range rdf:resource="http://www.w3.org/2001/XMLSchema#boolean"/>
        <rdfs:comment xml:lang="en">True if this Work is part of a series. In which case it should have a :workSeriesNumber</rdfs:comment>
        <rdfs:label xml:lang="en">is numbered</rdfs:label>
    </owl:DatatypeProperty>
    


    <!-- http://purl.bdrc.io/ontology/workIsbn -->

    <owl:DatatypeProperty rdf:about="http://purl.bdrc.io/ontology/workIsbn">
        <rdfs:domain rdf:resource="http://purl.bdrc.io/ontology/Work"/>
        <rdfs:range rdf:resource="http://purl.bdrc.io/ontology/ISBN"/>
        <admin:convertProperty xml:lang="en">convert to Bibframe identifiedBy with range Bibframe Isbn class</admin:convertProperty>
        <admin:convertToProperty rdf:resource="http://id.loc.gov/ontologies/bibframe/identifiedBy"/>
        <admin:convertValueToClass rdf:resource="http://id.loc.gov/ontologies/bibframe/Isbn"/>
        <rdfs:comment xml:lang="en">Refers to the International Standard Book Number for the Work</rdfs:comment>
        <rdfs:label xml:lang="en">has ISBN</rdfs:label>
    </owl:DatatypeProperty>
    


    <!-- http://purl.bdrc.io/ontology/workKaTenRefToh -->

    <owl:DatatypeProperty rdf:about="http://purl.bdrc.io/ontology/workKaTenRefToh">
        <rdfs:subPropertyOf rdf:resource="http://purl.bdrc.io/ontology/workRefs"/>
        <rdfs:domain rdf:resource="http://purl.bdrc.io/ontology/WorkRefs"/>
        <rdfs:range rdf:resource="http://www.w3.org/2001/XMLSchema#string"/>
        <rdfs:comment xml:lang="en">Tohoku Derge Kanjur and Tengyur Catalogue reference number</rdfs:comment>
        <rdfs:label xml:lang="en">toh number</rdfs:label>
        <rdfs:seeAlso rdf:resource="http://prajnaquest.fr/blog/tohoku-catalogue-available-here/"/>
    </owl:DatatypeProperty>
    


    <!-- http://purl.bdrc.io/ontology/workKaTenRefrKTs -->

    <owl:DatatypeProperty rdf:about="http://purl.bdrc.io/ontology/workKaTenRefrKTs">
        <rdfs:subPropertyOf rdf:resource="http://purl.bdrc.io/ontology/workRefs"/>
        <rdfs:domain rdf:resource="http://purl.bdrc.io/ontology/WorkRefs"/>
        <rdfs:range rdf:resource="http://www.w3.org/2001/XMLSchema#string"/>
        <rdfs:comment xml:lang="en">University of Vienna, resources for Kanju and Tanjur studies (rKTs) reference number</rdfs:comment>
        <rdfs:label xml:lang="en">rKTs reference</rdfs:label>
        <rdfs:seeAlso rdf:resource="https://www.istb.univie.ac.at/kanjur/xml4/xml/"/>
    </owl:DatatypeProperty>
    


    <!-- http://purl.bdrc.io/ontology/workKaTenSiglaBon -->

    <owl:DatatypeProperty rdf:about="http://purl.bdrc.io/ontology/workKaTenSiglaBon">
        <rdfs:subPropertyOf rdf:resource="http://purl.bdrc.io/ontology/workRefs"/>
        <rdfs:domain rdf:resource="http://purl.bdrc.io/ontology/WorkRefs"/>
        <rdfs:range rdf:resource="http://www.w3.org/2001/XMLSchema#string"/>
        <rdfs:comment xml:lang="en">Reference number in the Bon combined Kanjur and Tenjur</rdfs:comment>
        <rdfs:label xml:lang="en">bon kanjur item number</rdfs:label>
    </owl:DatatypeProperty>
    


    <!-- http://purl.bdrc.io/ontology/workKaTenSiglaD -->

    <owl:DatatypeProperty rdf:about="http://purl.bdrc.io/ontology/workKaTenSiglaD">
        <rdfs:subPropertyOf rdf:resource="http://purl.bdrc.io/ontology/workRefs"/>
        <rdfs:domain rdf:resource="http://purl.bdrc.io/ontology/WorkRefs"/>
        <rdfs:range rdf:resource="http://www.w3.org/2001/XMLSchema#string"/>
        <rdfs:comment xml:lang="en">Dergé Kangyur and Tengyur reference numbers</rdfs:comment>
        <rdfs:label xml:lang="en">sde dge number</rdfs:label>
        <rdfs:seeAlso rdf:resource="https://www.istb.univie.ac.at/kanjur/xml4/sub/sigla.php"/>
    </owl:DatatypeProperty>
    


    <!-- http://purl.bdrc.io/ontology/workKaTenSiglaG -->

    <owl:DatatypeProperty rdf:about="http://purl.bdrc.io/ontology/workKaTenSiglaG">
        <rdfs:subPropertyOf rdf:resource="http://purl.bdrc.io/ontology/workRefs"/>
        <rdfs:domain rdf:resource="http://purl.bdrc.io/ontology/WorkRefs"/>
        <rdfs:range rdf:resource="http://www.w3.org/2001/XMLSchema#string"/>
        <rdfs:comment xml:lang="en">Ganden (dga’ ldan) or “Golden Manuscript” (gser bris ma) Tengyur reference number</rdfs:comment>
        <rdfs:label xml:lang="en">gser bris number</rdfs:label>
        <rdfs:seeAlso rdf:resource="https://www.istb.univie.ac.at/kanjur/xml4/sub/sigla.php"/>
    </owl:DatatypeProperty>
    


    <!-- http://purl.bdrc.io/ontology/workKaTenSiglaH -->

    <owl:DatatypeProperty rdf:about="http://purl.bdrc.io/ontology/workKaTenSiglaH">
        <rdfs:subPropertyOf rdf:resource="http://purl.bdrc.io/ontology/workRefs"/>
        <rdfs:domain rdf:resource="http://purl.bdrc.io/ontology/WorkRefs"/>
        <rdfs:range rdf:resource="http://www.w3.org/2001/XMLSchema#string"/>
        <rdfs:comment xml:lang="en">Lhasa Kanjur reference number</rdfs:comment>
        <rdfs:label xml:lang="en">lhasa number</rdfs:label>
        <rdfs:seeAlso rdf:resource="https://www.istb.univie.ac.at/kanjur/xml4/sub/sigla.php"/>
    </owl:DatatypeProperty>
    


    <!-- http://purl.bdrc.io/ontology/workKaTenSiglaN -->

    <owl:DatatypeProperty rdf:about="http://purl.bdrc.io/ontology/workKaTenSiglaN">
        <rdfs:subPropertyOf rdf:resource="http://purl.bdrc.io/ontology/workRefs"/>
        <rdfs:domain rdf:resource="http://purl.bdrc.io/ontology/WorkRefs"/>
        <rdfs:range rdf:resource="http://www.w3.org/2001/XMLSchema#string"/>
        <rdfs:comment xml:lang="en">Narthang Kangyur and Tengyur reference number</rdfs:comment>
        <rdfs:label xml:lang="en">narthang number</rdfs:label>
    </owl:DatatypeProperty>
    


    <!-- http://purl.bdrc.io/ontology/workKaTenSiglaQ -->

    <owl:DatatypeProperty rdf:about="http://purl.bdrc.io/ontology/workKaTenSiglaQ">
        <rdfs:subPropertyOf rdf:resource="http://purl.bdrc.io/ontology/workRefs"/>
        <rdfs:domain rdf:resource="http://purl.bdrc.io/ontology/WorkRefs"/>
        <rdfs:range rdf:resource="http://www.w3.org/2001/XMLSchema#string"/>
        <rdfs:comment xml:lang="en">Reference numbers based on Beijing printed Kangyur and Tenjur. Conventional sigla, Q.</rdfs:comment>
        <rdfs:label xml:lang="en">otani beijing reference</rdfs:label>
        <rdfs:seeAlso rdf:resource="https://www.istb.univie.ac.at/kanjur/xml4/sub/sigla.php"/>
    </owl:DatatypeProperty>
    


    <!-- http://purl.bdrc.io/ontology/workKaTenSiglaS -->

    <owl:DatatypeProperty rdf:about="http://purl.bdrc.io/ontology/workKaTenSiglaS">
        <rdfs:subPropertyOf rdf:resource="http://purl.bdrc.io/ontology/workRefs"/>
        <rdfs:domain rdf:resource="http://purl.bdrc.io/ontology/WorkRefs"/>
        <rdfs:range rdf:resource="http://www.w3.org/2001/XMLSchema#string"/>
        <rdfs:comment xml:lang="en">Tok Palace manuscript Kanjur reference number</rdfs:comment>
        <rdfs:label xml:lang="en">stog number</rdfs:label>
        <rdfs:seeAlso rdf:resource="https://www.istb.univie.ac.at/kanjur/xml4/sub/sigla.php"/>
    </owl:DatatypeProperty>
    


    <!-- http://purl.bdrc.io/ontology/workKaTenSiglaU -->

    <owl:DatatypeProperty rdf:about="http://purl.bdrc.io/ontology/workKaTenSiglaU">
        <rdfs:subPropertyOf rdf:resource="http://purl.bdrc.io/ontology/workRefs"/>
        <rdfs:domain rdf:resource="http://purl.bdrc.io/ontology/WorkRefs"/>
        <rdfs:range rdf:resource="http://www.w3.org/2001/XMLSchema#string"/>
        <rdfs:comment xml:lang="en">Urga or Ulan Bator manuscript Kangyur reference number</rdfs:comment>
        <rdfs:label xml:lang="en">urga number</rdfs:label>
        <rdfs:seeAlso rdf:resource="https://www.istb.univie.ac.at/kanjur/xml4/sub/sigla.php"/>
    </owl:DatatypeProperty>
    


    <!-- http://purl.bdrc.io/ontology/workKaTenSiglaZ -->

    <owl:DatatypeProperty rdf:about="http://purl.bdrc.io/ontology/workKaTenSiglaZ">
        <rdfs:subPropertyOf rdf:resource="http://purl.bdrc.io/ontology/workRefs"/>
        <rdfs:domain rdf:resource="http://purl.bdrc.io/ontology/WorkRefs"/>
        <rdfs:range rdf:resource="http://www.w3.org/2001/XMLSchema#string"/>
        <rdfs:comment xml:lang="en">Shey Palace manuscript reference number</rdfs:comment>
        <rdfs:label xml:lang="en">shey number</rdfs:label>
        <rdfs:seeAlso rdf:resource="https://www.istb.univie.ac.at/kanjur/xml4/sub/sigla.php"/>
    </owl:DatatypeProperty>
    


    <!-- http://purl.bdrc.io/ontology/workLcCallNumber -->

    <owl:DatatypeProperty rdf:about="http://purl.bdrc.io/ontology/workLcCallNumber">
        <rdfs:domain rdf:resource="http://purl.bdrc.io/ontology/Work"/>
        <rdfs:range rdf:resource="http://purl.bdrc.io/ontology/LCCallNumber"/>
        <admin:convertProperty xml:lang="en">convert to Bibframe identifiedBy with range Bibframe ShelfMarkLcc class</admin:convertProperty>
        <admin:convertToProperty rdf:resource="http://id.loc.gov/ontologies/bibframe/identifiedBy"/>
        <admin:convertValueToClass rdf:resource="http://id.loc.gov/ontologies/bibframe/ShelfMarkLcc"/>
        <rdfs:comment xml:lang="en">Refers to the Library of Congress Shelf mark call number</rdfs:comment>
        <rdfs:label xml:lang="en">has LC Call Number</rdfs:label>
    </owl:DatatypeProperty>
    


    <!-- http://purl.bdrc.io/ontology/workLccn -->

    <owl:DatatypeProperty rdf:about="http://purl.bdrc.io/ontology/workLccn">
        <rdfs:domain rdf:resource="http://purl.bdrc.io/ontology/Work"/>
        <rdfs:range rdf:resource="http://purl.bdrc.io/ontology/LCCN"/>
        <admin:convertProperty xml:lang="en">convert to Bibframe identifiedBy with range Bibframe Lccn class</admin:convertProperty>
        <admin:convertToProperty rdf:resource="http://id.loc.gov/ontologies/bibframe/identifiedBy"/>
        <admin:convertValueToClass rdf:resource="http://id.loc.gov/ontologies/bibframe/Lccn"/>
        <rdfs:comment xml:lang="en">Refers to the Library of Congress Control Number</rdfs:comment>
        <rdfs:label xml:lang="en">has LCCN</rdfs:label>
    </owl:DatatypeProperty>
    


    <!-- http://purl.bdrc.io/ontology/workLegacyNode -->

    <owl:DatatypeProperty rdf:about="http://purl.bdrc.io/ontology/workLegacyNode">
        <rdfs:domain rdf:resource="http://purl.bdrc.io/ontology/Work"/>
        <rdfs:range rdf:resource="http://www.w3.org/2001/XMLSchema#string"/>
        <rdfs:comment xml:lang="en">The value is the legacy Outline Node RID so that redirection can be implemented for purls referencing nodes on the old www.tbrc.org site.</rdfs:comment>
        <rdfs:label xml:lang="en">has legacy node</rdfs:label>
    </owl:DatatypeProperty>
    


    <!-- http://purl.bdrc.io/ontology/workLocationByFolio -->

    <owl:DatatypeProperty rdf:about="http://purl.bdrc.io/ontology/workLocationByFolio">
        <rdfs:domain rdf:resource="http://purl.bdrc.io/ontology/WorkLocation"/>
        <rdfs:range rdf:resource="http://www.w3.org/2001/XMLSchema#boolean"/>
        <rdfs:comment xml:lang="en">If true then the location is specified in terms of folio # and side: verso/recto</rdfs:comment>
        <rdfs:label xml:lang="en">location by folio</rdfs:label>
    </owl:DatatypeProperty>
    


    <!-- http://purl.bdrc.io/ontology/workLocationFF -->

    <owl:DatatypeProperty rdf:about="http://purl.bdrc.io/ontology/workLocationFF">
        <rdfs:domain rdf:resource="http://purl.bdrc.io/ontology/WorkLocation"/>
        <rdfs:range rdf:resource="http://www.w3.org/2001/XMLSchema#integer"/>
        <rdfs:comment xml:lang="en">Indicates the number of following pages included in the WorkLocation. This is an alternative to using bdr:WorkLocationBegins and bdr:WorkLocationEnds which are really only needed when a WorkLocation spans volumes or when there is a reason to specify begin and end locations down to the line and phrase, e.g., in some of the rGyud &apos;bum where texts start and end mid-page</rdfs:comment>
        <rdfs:label xml:lang="en">ff</rdfs:label>
    </owl:DatatypeProperty>
    


    <!-- http://purl.bdrc.io/ontology/workLocationLine -->

    <owl:DatatypeProperty rdf:about="http://purl.bdrc.io/ontology/workLocationLine">
        <rdfs:subPropertyOf rdf:resource="http://www.w3.org/2002/07/owl#topDataProperty"/>
        <rdfs:domain rdf:resource="http://purl.bdrc.io/ontology/WorkLocation"/>
        <rdfs:range>
            <rdfs:Datatype>
                <owl:unionOf rdf:parseType="Collection">
                    <rdf:Description rdf:about="http://www.w3.org/2001/XMLSchema#positiveInteger"/>
                    <rdf:Description rdf:about="http://www.w3.org/2001/XMLSchema#string"/>
                </owl:unionOf>
            </rdfs:Datatype>
        </rdfs:range>
        <rdfs:comment xml:lang="en">The line on the page that is referenced</rdfs:comment>
        <rdfs:label xml:lang="en">line</rdfs:label>
    </owl:DatatypeProperty>
    


    <!-- http://purl.bdrc.io/ontology/workLocationPage -->

    <owl:DatatypeProperty rdf:about="http://purl.bdrc.io/ontology/workLocationPage">
        <rdfs:subPropertyOf rdf:resource="http://www.w3.org/2002/07/owl#topDataProperty"/>
        <rdfs:domain rdf:resource="http://purl.bdrc.io/ontology/WorkLocation"/>
        <rdfs:range>
            <rdfs:Datatype>
                <owl:unionOf rdf:parseType="Collection">
                    <rdf:Description rdf:about="http://www.w3.org/2001/XMLSchema#positiveInteger"/>
                    <rdf:Description rdf:about="http://www.w3.org/2001/XMLSchema#string"/>
                </owl:unionOf>
            </rdfs:Datatype>
        </rdfs:range>
        <rdfs:comment xml:lang="en">The page in the volume of the Work indicated by the other statements for this :WorkLocation</rdfs:comment>
        <rdfs:label xml:lang="en">page</rdfs:label>
    </owl:DatatypeProperty>
    


    <!-- http://purl.bdrc.io/ontology/workLocationPhrase -->

    <owl:DatatypeProperty rdf:about="http://purl.bdrc.io/ontology/workLocationPhrase">
        <rdfs:subPropertyOf rdf:resource="http://www.w3.org/2002/07/owl#topDataProperty"/>
        <rdfs:range>
            <rdfs:Datatype>
                <owl:unionOf rdf:parseType="Collection">
                    <rdf:Description rdf:about="http://www.w3.org/2001/XMLSchema#positiveInteger"/>
                    <rdf:Description rdf:about="http://www.w3.org/2001/XMLSchema#string"/>
                </owl:unionOf>
            </rdfs:Datatype>
        </rdfs:range>
        <rdfs:comment xml:lang="en">This should be a positive integer counting from the left side of the page tshegs and shads to the phrase (syllable) that is to be indicated by the location. This is optional and only makes sense if there is a :workLocationLine specified as well.</rdfs:comment>
        <rdfs:label xml:lang="en">phrase</rdfs:label>
    </owl:DatatypeProperty>
    


    <!-- http://purl.bdrc.io/ontology/workLocationSide -->

    <owl:DatatypeProperty rdf:about="http://purl.bdrc.io/ontology/workLocationSide">
        <rdfs:subPropertyOf rdf:resource="http://www.w3.org/2002/07/owl#topDataProperty"/>
        <rdfs:domain rdf:resource="http://purl.bdrc.io/ontology/WorkLocation"/>
        <rdfs:range rdf:resource="http://www.w3.org/2001/XMLSchema#string"/>
        <rdfs:comment xml:lang="en">If :workLocationByFolio true then side should be either &quot;recto&quot; or &quot;verso&quot; but will likely need to be normalized since there has not been validation in the editor of this field. Most locations are specified in terms of pages.</rdfs:comment>
        <rdfs:label xml:lang="en">side</rdfs:label>
    </owl:DatatypeProperty>
    


    <!-- http://purl.bdrc.io/ontology/workLocationStatement -->

    <owl:DatatypeProperty rdf:about="http://purl.bdrc.io/ontology/workLocationStatement">
        <rdfs:domain rdf:resource="http://purl.bdrc.io/ontology/Work"/>
        <rdfs:range rdf:resource="http://www.w3.org/2001/XMLSchema#string"/>
        <rdfs:comment xml:lang="en">A statement of the location of this Work in a containing Work or of the pagination present in the text versus the formal location in terms of page images.</rdfs:comment>
        <rdfs:label xml:lang="en">location statement</rdfs:label>
    </owl:DatatypeProperty>
    


    <!-- http://purl.bdrc.io/ontology/workLocationVolume -->

    <owl:DatatypeProperty rdf:about="http://purl.bdrc.io/ontology/workLocationVolume">
        <rdfs:subPropertyOf rdf:resource="http://www.w3.org/2002/07/owl#topDataProperty"/>
        <rdfs:domain rdf:resource="http://purl.bdrc.io/ontology/WorkLocation"/>
        <rdfs:range>
            <rdfs:Datatype>
                <owl:unionOf rdf:parseType="Collection">
                    <rdf:Description rdf:about="http://www.w3.org/2001/XMLSchema#positiveInteger"/>
                    <rdf:Description rdf:about="http://www.w3.org/2001/XMLSchema#string"/>
                </owl:unionOf>
            </rdfs:Datatype>
        </rdfs:range>
        <rdfs:comment xml:lang="en">this should be a positive integer indicating the volume of the Work referenced in this Location</rdfs:comment>
        <rdfs:label xml:lang="en">volume</rdfs:label>
    </owl:DatatypeProperty>
    


    <!-- http://purl.bdrc.io/ontology/workNumberOfVolumes -->

    <owl:DatatypeProperty rdf:about="http://purl.bdrc.io/ontology/workNumberOfVolumes">
        <rdfs:range rdf:resource="http://www.w3.org/2001/XMLSchema#positiveInteger"/>
        <rdfs:comment xml:lang="en">Migration info: this is the &lt;work:archiveInfo @vols/&gt; attribute.</rdfs:comment>
        <rdfs:comment xml:lang="en">This is the number of volumes (if any) associated with the Work. Typically this is for a published work. The value may differ from the &quot;actual&quot; number of volumes in an associated Item owing to missing volumes.</rdfs:comment>
        <rdfs:label xml:lang="en">number of volumes</rdfs:label>
    </owl:DatatypeProperty>
    


    <!-- http://purl.bdrc.io/ontology/workPL480 -->

    <owl:DatatypeProperty rdf:about="http://purl.bdrc.io/ontology/workPL480">
        <rdfs:domain rdf:resource="http://purl.bdrc.io/ontology/Work"/>
        <rdfs:range rdf:resource="http://www.w3.org/2001/XMLSchema#string"/>
    </owl:DatatypeProperty>
    


    <!-- http://purl.bdrc.io/ontology/workPrintery -->

    <owl:DatatypeProperty rdf:about="http://purl.bdrc.io/ontology/workPrintery">
        <rdfs:domain rdf:resource="http://purl.bdrc.io/ontology/Work"/>
        <rdfs:range rdf:resource="http://www.w3.org/1999/02/22-rdf-syntax-ns#PlainLiteral"/>
    </owl:DatatypeProperty>
    


    <!-- http://purl.bdrc.io/ontology/workPubinfoVolumes -->

    <owl:DatatypeProperty rdf:about="http://purl.bdrc.io/ontology/workPubinfoVolumes">
        <rdfs:domain rdf:resource="http://purl.bdrc.io/ontology/Work"/>
        <rdfs:range rdf:resource="http://www.w3.org/2001/XMLSchema#string"/>
    </owl:DatatypeProperty>
    


    <!-- http://purl.bdrc.io/ontology/workPublisherDate -->

    <owl:DatatypeProperty rdf:about="http://purl.bdrc.io/ontology/workPublisherDate">
        <rdfs:domain rdf:resource="http://purl.bdrc.io/ontology/Work"/>
        <rdfs:range rdf:resource="http://www.w3.org/2001/XMLSchema#string"/>
    </owl:DatatypeProperty>
    


    <!-- http://purl.bdrc.io/ontology/workPublisherLocation -->

    <owl:DatatypeProperty rdf:about="http://purl.bdrc.io/ontology/workPublisherLocation">
        <rdfs:domain rdf:resource="http://purl.bdrc.io/ontology/Work"/>
        <rdfs:range rdf:resource="http://www.w3.org/1999/02/22-rdf-syntax-ns#PlainLiteral"/>
    </owl:DatatypeProperty>
    


    <!-- http://purl.bdrc.io/ontology/workPublisherName -->

    <owl:DatatypeProperty rdf:about="http://purl.bdrc.io/ontology/workPublisherName">
        <rdfs:domain rdf:resource="http://purl.bdrc.io/ontology/Work"/>
        <rdfs:range rdf:resource="http://www.w3.org/1999/02/22-rdf-syntax-ns#PlainLiteral"/>
    </owl:DatatypeProperty>
    


    <!-- http://purl.bdrc.io/ontology/workRefChokLing -->

    <owl:DatatypeProperty rdf:about="http://purl.bdrc.io/ontology/workRefChokLing">
        <rdfs:subPropertyOf rdf:resource="http://purl.bdrc.io/ontology/workRefs"/>
        <rdfs:domain rdf:resource="http://purl.bdrc.io/ontology/WorkRefs"/>
        <rdfs:range rdf:resource="http://www.w3.org/2001/XMLSchema#string"/>
        <rdfs:comment xml:lang="en">Catalogue of the New Treasures of Chokgyur Lingpa reference used only in cataloguing parts of bdr:W22642</rdfs:comment>
        <rdfs:label xml:lang="en">chokling tersar reference</rdfs:label>
        <rdfs:seeAlso rdf:resource="http://rywiki.tsadra.org/index.php/Catalogue_of_the_New_Treasures_of_Chokgyur_Lingpa_Part_1"/>
    </owl:DatatypeProperty>
    


    <!-- http://purl.bdrc.io/ontology/workRefIsIAO -->

    <owl:DatatypeProperty rdf:about="http://purl.bdrc.io/ontology/workRefIsIAO">
        <rdfs:subPropertyOf rdf:resource="http://purl.bdrc.io/ontology/workRefs"/>
        <rdfs:domain rdf:resource="http://purl.bdrc.io/ontology/WorkRefs"/>
        <rdfs:range rdf:resource="http://www.w3.org/2001/XMLSchema#string"/>
        <rdfs:comment xml:lang="en">Catalog of the Tucci Tibetan fund in the library of ISMEO</rdfs:comment>
        <rdfs:label xml:lang="en">IsIAO reference</rdfs:label>
        <rdfs:seeAlso rdf:resource="https://www.tbrc.org/#!rid=W19841"/>
    </owl:DatatypeProperty>
    


    <!-- http://purl.bdrc.io/ontology/workRefs -->

    <owl:DatatypeProperty rdf:about="http://purl.bdrc.io/ontology/workRefs">
        <rdfs:domain rdf:resource="http://purl.bdrc.io/ontology/WorkRefs"/>
        <rdfs:comment xml:lang="en">This Data property groups together all of the various reference number properties derived from various catalogues and such. This property can be used by an editor to easily locate all of the possible reference number properties that might need to be used during cataloguing.</rdfs:comment>
        <rdfs:label xml:lang="en">reference numbers</rdfs:label>
    </owl:DatatypeProperty>
    


    <!-- http://purl.bdrc.io/ontology/workScanInfo -->

    <owl:DatatypeProperty rdf:about="http://purl.bdrc.io/ontology/workScanInfo">
        <rdfs:domain rdf:resource="http://purl.bdrc.io/ontology/Work"/>
        <rdfs:range rdf:resource="http://www.w3.org/1999/02/22-rdf-syntax-ns#PlainLiteral"/>
    </owl:DatatypeProperty>
    


    <!-- http://purl.bdrc.io/ontology/workSeeHarvard -->

    <owl:DatatypeProperty rdf:about="http://purl.bdrc.io/ontology/workSeeHarvard">
        <rdfs:domain rdf:resource="http://purl.bdrc.io/ontology/Work"/>
        <rdfs:range rdf:resource="http://www.w3.org/2001/XMLSchema#string"/>
    </owl:DatatypeProperty>
    


    <!-- http://purl.bdrc.io/ontology/workSeriesContent -->

    <owl:DatatypeProperty rdf:about="http://purl.bdrc.io/ontology/workSeriesContent">
        <rdfs:domain rdf:resource="http://purl.bdrc.io/ontology/WorkPubinfoSeries"/>
        <rdfs:range rdf:resource="http://www.w3.org/1999/02/22-rdf-syntax-ns#PlainLiteral"/>
    </owl:DatatypeProperty>
    


    <!-- http://purl.bdrc.io/ontology/workSeriesName -->

    <owl:DatatypeProperty rdf:about="http://purl.bdrc.io/ontology/workSeriesName">
        <rdfs:domain rdf:resource="http://purl.bdrc.io/ontology/WorkPubinfoSeries"/>
        <rdfs:range rdf:resource="http://www.w3.org/1999/02/22-rdf-syntax-ns#PlainLiteral"/>
    </owl:DatatypeProperty>
    


    <!-- http://purl.bdrc.io/ontology/workSeriesNumber -->

    <owl:DatatypeProperty rdf:about="http://purl.bdrc.io/ontology/workSeriesNumber">
        <rdfs:domain rdf:resource="http://purl.bdrc.io/ontology/Work"/>
        <rdfs:domain rdf:resource="http://purl.bdrc.io/ontology/WorkPubinfoSeries"/>
        <rdfs:range rdf:resource="http://www.w3.org/2001/XMLSchema#string"/>
        <rdfs:comment xml:lang="en">This is the number of this Work in a series - implies that this work is a part (member of) a series Work.</rdfs:comment>
        <rdfs:label xml:lang="en">number</rdfs:label>
    </owl:DatatypeProperty>
    


    <!-- http://purl.bdrc.io/ontology/workSourceNote -->

    <owl:DatatypeProperty rdf:about="http://purl.bdrc.io/ontology/workSourceNote">
        <rdfs:domain rdf:resource="http://purl.bdrc.io/ontology/Work"/>
        <rdfs:range rdf:resource="http://www.w3.org/1999/02/22-rdf-syntax-ns#PlainLiteral"/>
    </owl:DatatypeProperty>
    


    <!-- http://purl.bdrc.io/ontology/workSourcePrintery_string -->

    <owl:DatatypeProperty rdf:about="http://purl.bdrc.io/ontology/workSourcePrintery_string">
        <rdfs:domain rdf:resource="http://purl.bdrc.io/ontology/Work"/>
        <rdfs:range rdf:resource="http://www.w3.org/2001/XMLSchema#string"/>
    </owl:DatatypeProperty>
    


    <!-- http://purl.bdrc.io/ontology/work_desc_id -->

    <owl:DatatypeProperty rdf:about="http://purl.bdrc.io/ontology/work_desc_id">
        <rdfs:domain rdf:resource="http://purl.bdrc.io/ontology/Work"/>
        <rdfs:range rdf:resource="http://www.w3.org/2001/XMLSchema#string"/>
        <rdfs:comment xml:lang="en">used in the Fragile Palm Leaves project in &lt;w:description type=&quot;id&quot;/&gt;</rdfs:comment>
        <rdfs:label xml:lang="en">id</rdfs:label>
    </owl:DatatypeProperty>
    


    <!-- http://purl.bdrc.io/ontology/work_desc_remarks -->

    <owl:DatatypeProperty rdf:about="http://purl.bdrc.io/ontology/work_desc_remarks">
        <rdfs:domain rdf:resource="http://purl.bdrc.io/ontology/Work"/>
        <rdfs:range rdf:resource="http://www.w3.org/2001/XMLSchema#string"/>
        <rdfs:comment xml:lang="en">used in the Fragile Palm Leaves project in &lt;w:description type=&quot;remarks&quot;/&gt;</rdfs:comment>
        <rdfs:label xml:lang="en">remarks</rdfs:label>
    </owl:DatatypeProperty>
    


    <!-- http://purl.bdrc.io/ontology/work_desc_room -->

    <owl:DatatypeProperty rdf:about="http://purl.bdrc.io/ontology/work_desc_room">
        <rdfs:domain rdf:resource="http://purl.bdrc.io/ontology/Work"/>
        <rdfs:range rdf:resource="http://www.w3.org/2001/XMLSchema#string"/>
        <rdfs:comment xml:lang="en">used in the Fragile Palm Leaves project in &lt;w:description type=&quot;room&quot;/&gt;</rdfs:comment>
        <rdfs:label xml:lang="en">room</rdfs:label>
    </owl:DatatypeProperty>
    


    <!-- 
    ///////////////////////////////////////////////////////////////////////////////////////
    //
    // Classes
    //
    ///////////////////////////////////////////////////////////////////////////////////////
     -->

    


    <!-- http://id.loc.gov/ontologies/bibframe/Identifier -->

    <owl:Class rdf:about="http://id.loc.gov/ontologies/bibframe/Identifier">
        <rdfs:subClassOf rdf:resource="http://id.loc.gov/ontologies/bibframe/Thing"/>
        <rdfs:comment xml:lang="en">Token or name that is associated with a resource, such as a URI or an ISBN.</rdfs:comment>
        <rdfs:label xml:lang="en">Bibframe Identifier</rdfs:label>
    </owl:Class>
    


    <!-- http://id.loc.gov/ontologies/bibframe/Isbn -->

    <owl:Class rdf:about="http://id.loc.gov/ontologies/bibframe/Isbn">
        <rdfs:subClassOf rdf:resource="http://id.loc.gov/ontologies/bibframe/Identifier"/>
        <rdfs:comment xml:lang="en">International Standard Book Number.</rdfs:comment>
        <rdfs:label xml:lang="en">ISBN</rdfs:label>
    </owl:Class>
    


    <!-- http://id.loc.gov/ontologies/bibframe/Lccn -->

    <owl:Class rdf:about="http://id.loc.gov/ontologies/bibframe/Lccn">
        <rdfs:subClassOf rdf:resource="http://id.loc.gov/ontologies/bibframe/Identifier"/>
        <rdfs:comment xml:lang="en">Library of Congress Control Number that identifies a resource description.</rdfs:comment>
        <rdfs:label xml:lang="en">LCCN</rdfs:label>
    </owl:Class>
    


    <!-- http://id.loc.gov/ontologies/bibframe/ShelfMarkLcc -->

    <owl:Class rdf:about="http://id.loc.gov/ontologies/bibframe/ShelfMarkLcc">
        <rdfs:subClassOf rdf:resource="http://id.loc.gov/ontologies/bibframe/Identifier"/>
        <rdfs:comment xml:lang="en">Shelf mark based on Library of Congress Classification.</rdfs:comment>
        <rdfs:label xml:lang="en">LCC call number</rdfs:label>
    </owl:Class>
    


    <!-- http://id.loc.gov/ontologies/bibframe/Thing -->

    <owl:Class rdf:about="http://id.loc.gov/ontologies/bibframe/Thing">
        <rdfs:comment xml:lang="en">subclasses of bf:Thing are bibframe classes that are referred to in the bdrc ontology</rdfs:comment>
        <rdfs:label xml:lang="en">Bibframe Thing</rdfs:label>
    </owl:Class>
    


    <!-- http://purl.bdrc.io/ontology/Corporation -->

    <owl:Class rdf:about="http://purl.bdrc.io/ontology/Corporation">
        <rdfs:subClassOf rdf:resource="http://purl.bdrc.io/ontology/Entity"/>
        <rdfs:comment xml:lang="en">Corporations include families, political groups, religous groups, business entities and so on. A more neutral label for the class would be Organziation</rdfs:comment>
        <rdfs:comment xml:lang="en">Names are represented by rdfs:label</rdfs:comment>
        <rdfs:label xml:lang="en">Corporation</rdfs:label>
    </owl:Class>
    


    <!-- http://purl.bdrc.io/ontology/CorporationMember -->

    <owl:Class rdf:about="http://purl.bdrc.io/ontology/CorporationMember">
        <rdfs:subClassOf rdf:resource="http://purl.bdrc.io/ontology/Facet"/>
        <rdfs:comment xml:lang="en">Describes a member of the subject Corporation by indicating the :Person that is a member and the :CorporationMemberType of the :Person:

bdr:Czzzz a :Corporation ;
                 :corporationHasMember
                       [ a :CorporationMember ;
                         :corporationMember bdr:Pyyyyy ;
                         :corporationMemberType bdr:CorporationMemberTypeByBlood ] ;
                 :corporationHasMember
                       [ a CorporationMember ;
                         :corporationMember bdr:Pxxxxx ;
                         :corporationMemberType bdr:CorporationMemberTypeByMarriage ] .</rdfs:comment>
        <rdfs:label xml:lang="en">Corporation Member</rdfs:label>
    </owl:Class>
    


    <!-- http://purl.bdrc.io/ontology/CorporationMemberType -->

    <owl:Class rdf:about="http://purl.bdrc.io/ontology/CorporationMemberType">
        <rdfs:subClassOf rdf:resource="http://purl.bdrc.io/ontology/Type"/>
        <rdfs:comment xml:lang="en">Indicates the relation of a given :Person to the corporation, such as related by blood, marriage, or monastic status</rdfs:comment>
        <rdfs:label xml:lang="en">Corporation Member type</rdfs:label>
    </owl:Class>
    


    <!-- http://purl.bdrc.io/ontology/Entity -->

    <owl:Class rdf:about="http://purl.bdrc.io/ontology/Entity">
        <rdfs:comment xml:lang="en">Entities are the principle types or concepts of the bdrc ontology. Generally individuals of type a subclass of :Entity will correspond to distinct individuals in the domain of discourse of bdrc. So Persons, Places, Works and so on will correspond to historical, mythical or contemporaneous individuals (instances in object-oriented terms).</rdfs:comment>
        <rdfs:label xml:lang="en">Entity</rdfs:label>
    </owl:Class>
    


    <!-- http://purl.bdrc.io/ontology/External -->

    <owl:Class rdf:about="http://purl.bdrc.io/ontology/External">
        <rdfs:subClassOf rdf:resource="http://purl.bdrc.io/ontology/Facet"/>
        <rdfs:subClassOf>
            <owl:Restriction>
                <owl:onProperty rdf:resource="http://purl.bdrc.io/ontology/external_data"/>
                <owl:qualifiedCardinality rdf:datatype="http://www.w3.org/2001/XMLSchema#nonNegativeInteger">1</owl:qualifiedCardinality>
                <owl:onDataRange rdf:resource="http://www.w3.org/2001/XMLSchema#anyURI"/>
            </owl:Restriction>
        </rdfs:subClassOf>
        <rdfs:subClassOf>
            <owl:Restriction>
                <owl:onProperty rdf:resource="http://purl.bdrc.io/ontology/external_source"/>
                <owl:qualifiedCardinality rdf:datatype="http://www.w3.org/2001/XMLSchema#nonNegativeInteger">1</owl:qualifiedCardinality>
                <owl:onDataRange rdf:resource="http://www.w3.org/2001/XMLSchema#anyURI"/>
            </owl:Restriction>
        </rdfs:subClassOf>
        <rdfs:comment>The external entry element is intended to be used to link to an external site / resource that provides additional or related information for the Work, Person, Place and so on. The content of the external entry is a string that will be displayed by the web client. If the data attribute is present it will be interpreted as a URL linking to a web resource, e.g., to a related Treasury of Lives biography. There are currently a few records, e.g., G1KG5700, that have data links to TBRC Outline nodes.

If the data attribute is present the web-client will use it to display a link that can be clicked to visit the linked item in a new window.</rdfs:comment>
    </owl:Class>
    


    <!-- http://purl.bdrc.io/ontology/Facet -->

    <owl:Class rdf:about="http://purl.bdrc.io/ontology/Facet">
        <rdfs:comment xml:lang="en">:Facets are essentially n-ary relations that apply to one or more Resources. Facets are compound features or properties of Resources.</rdfs:comment>
        <rdfs:label xml:lang="en">Facet</rdfs:label>
    </owl:Class>
    


    <!-- http://purl.bdrc.io/ontology/Gender -->

    <owl:Class rdf:about="http://purl.bdrc.io/ontology/Gender">
        <rdfs:subClassOf rdf:resource="http://purl.bdrc.io/ontology/Type"/>
        <rdfs:comment xml:lang="en">Records the gender of a :Person if known; otherwise, bdr:GenderNotSpecified</rdfs:comment>
        <rdfs:label xml:lang="en">Gender</rdfs:label>
    </owl:Class>
    


    <!-- http://purl.bdrc.io/ontology/Item -->

    <owl:Class rdf:about="http://purl.bdrc.io/ontology/Item">
        <rdfs:subClassOf rdf:resource="http://purl.bdrc.io/ontology/Entity"/>
        <rdfs:comment xml:lang="en">ScanRequest for the Work associated with an :Item is migrated as :scan_venue, and the instructions note (if any) attached to the ScanRequest. The work attribute of scanrequest refers to the work for the volumes object  all other fields of scanrequest are ignored for migration</rdfs:comment>
        <rdfs:comment xml:lang="en">The :Item resource collects info from ImageGroups and Scan-Requests. An :Item is a collection of :Volume components for each volume in the associated :Work. Each :Volume MAY have a :onDisk property which will have a &apos;|&apos; separated list of names of the page image files. This property is present when the subject volume has been digitized and deposited in the online archive.</rdfs:comment>
        <rdfs:label xml:lang="en">Item</rdfs:label>
    </owl:Class>
    


    <!-- http://purl.bdrc.io/ontology/ItemType -->

    <owl:Class rdf:about="http://purl.bdrc.io/ontology/ItemType">
        <rdfs:subClassOf rdf:resource="http://purl.bdrc.io/ontology/Type"/>
        <rdfs:comment xml:lang="en">The type of Item: scanned asset, ocr&apos;d, physical holding, etc</rdfs:comment>
        <rdfs:label xml:lang="en">item type</rdfs:label>
    </owl:Class>
    


    <!-- http://purl.bdrc.io/ontology/Kin -->

    <owl:Class rdf:about="http://purl.bdrc.io/ontology/Kin">
        <rdfs:subClassOf rdf:resource="http://purl.bdrc.io/ontology/Facet"/>
        <rdfs:comment xml:lang="en">A :Kin facet describes a kinship relation between the subject :Person and some other :Person:

bdr:Pxxxx a :Person ;
                 :personHasKin [ a :Kin ;
                                           :personKinType bdr:KinUncle ;
                                           :personKinWho bdr:Pyyyy ]</rdfs:comment>
        <rdfs:label xml:lang="en">Kin</rdfs:label>
    </owl:Class>
    


    <!-- http://purl.bdrc.io/ontology/KinType -->

    <owl:Class rdf:about="http://purl.bdrc.io/ontology/KinType">
        <rdfs:subClassOf rdf:resource="http://purl.bdrc.io/ontology/Type"/>
        <rdfs:comment xml:lang="en">Indicates the kin relation of one person to another, such as, brother, parent, child and so on.</rdfs:comment>
        <rdfs:label xml:lang="en">Kin</rdfs:label>
    </owl:Class>
    


    <!-- http://purl.bdrc.io/ontology/Lineage -->

    <owl:Class rdf:about="http://purl.bdrc.io/ontology/Lineage">
        <rdfs:subClassOf rdf:resource="http://purl.bdrc.io/ontology/Entity"/>
        <inferSubTree rdf:datatype="http://www.w3.org/2001/XMLSchema#boolean">true</inferSubTree>
        <rdfs:comment xml:lang="en">Example:

bdr:L8LS15684 a :Lineage ; :status bdr:StatusReleased ;
      rdfs:label &quot;mngon rtogs rgyan gyi &apos;grel pa don gsal gyi brgyud pa/&quot;@bo-x-ewts ;
      :lineageType bdr:LineageLung ;
      :lineageObject bdr:W21662 ;
      :lineageObject bdr:T36 ;
      :lineageLocation [ a :WorkLocation ;
            :workLocationPage &quot;131&quot; ;
            :workLocationVolume &quot;1&quot; ;
            :workLocationWork bdr:W1KG16278 ]
      :lineageHolder [ a :LineageHolder ;
            :lineageWho bdr:T10MS11142 ]
      :lineageHolder [ a :LineageHolder ;
            :lineageWho bdr:T681 ;
            :lineageReceived [ a :LineageReceived ;
                  :lineageFrom bdr:T10MS11142 ]
            ]
      :lineageHolder [ a :LineageHolder ;
            :lineageWho bdr:P6117 ;
            :lineageReceived [ a :LineageReceived ;
                  :lineageFrom bdr:T681 ]
            ]</rdfs:comment>
        <rdfs:comment xml:lang="en">Lineages represent information about how a particular text or group of texts or perhaps purely oral transmission has been passed from one individual to another. The Tibetan genres, gsan yig and thob yig.

Lineage transmissions capture the relationship between lineage holders, sets of texts and the places and dates where/when the lineage was transferred from one holder to another.</rdfs:comment>
        <rdfs:comment xml:lang="en">Names are represented by rdfs:label</rdfs:comment>
        <rdfs:label xml:lang="en">Lineage</rdfs:label>
        <rdfs:seeAlso rdf:resource="https://link.springer.com/article/10.1023%2FA%3A1004844115222?LI=true"/>
    </owl:Class>
    


    <!-- http://purl.bdrc.io/ontology/LineageAlternative -->

    <owl:Class rdf:about="http://purl.bdrc.io/ontology/LineageAlternative">
        <rdfs:subClassOf rdf:resource="http://purl.bdrc.io/ontology/Facet"/>
        <owl:deprecated xml:lang="en">An Alternative was intended to be used to express a variant of the main lineage &quot;inline&quot; in the same Lineage document rather than creating separate documents for each lineage variation. 

It is modeled on the conventions used in gsan yig for this purpose. So an Alternative will typically have three or more holders: 
    1) the start holder that mentions a holder in the containing Lineage that is the start point of the variation; 
    2) then one or more holders that represent the variation; and
    3) then a final holder that mentions a holder in the containing Lineage that is the end point of the variation. 

The start holder is marked by including a downTo element and the end holder is marked with a downFrom element. If the downTo holder is not present then the variation is a variation on the intial sequence of the lineage. If the downFrom is not present then the variation is a the end of the lineage. 

Generally the Alternatives should appear at the end of the main sequence of holders and there may be as many Alternatives as needed to express the variations in the gsan yig / thob yig.</owl:deprecated>
        <owl:deprecated xml:lang="en">This feature is not used. There are two empty occurrences of &lt;lin:alternative/&gt; in L1RKL1802.xml and
L1RKL1822.xml.

The :lineageRef is used instead to refer to a separate :Lineage rather than adding undue complexity to the modeling of :Lineage.</owl:deprecated>
    </owl:Class>
    


    <!-- http://purl.bdrc.io/ontology/LineageHolder -->

    <owl:Class rdf:about="http://purl.bdrc.io/ontology/LineageHolder">
        <rdfs:subClassOf rdf:resource="http://purl.bdrc.io/ontology/Facet"/>
        <rdfs:comment xml:lang="en">A :LineageHolder describes a :Person or other :Entity (i.e., a deity or mythical being) that was/is considered to be the authoritative transmitter of a :Lineage.

Usually the holder received the :Lineage from some other entity but there is a &quot;first&quot; holder who counts as the original holder of the :Lineage.

A holder may create/author one or more Works concerning the Lineage and these are included with the holder as well as the, usually unique, prior holder of the lineage who transmitted it on to the current holder.

The :LineageReceived records the entity from whom the :Lineage was received, as well as the :Place where the :Lineage was transmitted to the current holder and the circa of the transmission if known.

For example,

bdr:Lwwww a :Lineage ;
                   :lineageHolder
                       [ a :LineageHolder ;
                         :lineageWho bdr:Paaaa ;
                         :lineageReceived
                              [ a :LineageReceived ;
                                :lineageFrom bdr:Pbbbb ;
                                :lineageSite bdr:Gdddd ;
                                :onOrAbout 134u ] ;
                          :lineageWork bdr:Wcccc ]</rdfs:comment>
        <rdfs:label xml:lang="en">lineage holder</rdfs:label>
    </owl:Class>
    


    <!-- http://purl.bdrc.io/ontology/LineageReceived -->

    <owl:Class rdf:about="http://purl.bdrc.io/ontology/LineageReceived">
        <rdfs:subClassOf rdf:resource="http://purl.bdrc.io/ontology/Facet"/>
        <rdfs:comment xml:lang="en">Each :LineageReceived describes another :LineageHolder from whom the current :LineageHolder received the :Lineage transmission. Typically there is a unique :LineageHolder from whom the :Lineage is received but two or more are possible.

For example,

bdr:Lwwww a :Lineage ;
                   :lineageHolder
                       [ a :LineageHolder ;
                         :lineageWho bdr:Paaaa ;
                         :lineageReceived
                              [ a :LineageReceived ;
                                :lineageFrom bdr:Pbbbb ;
                                :lineageSite bdr:Gdddd ;
                                :onOrAbout &quot;134u&quot; ] ;
                          :lineageWork bdr:Wcccc ]</rdfs:comment>
        <rdfs:seeAlso rdf:resource="http://purl.bdrc.io/ontology/LineageHolder"/>
    </owl:Class>
    


    <!-- http://purl.bdrc.io/ontology/LineageType -->

    <owl:Class rdf:about="http://purl.bdrc.io/ontology/LineageType">
        <rdfs:subClassOf rdf:resource="http://purl.bdrc.io/ontology/Type"/>
        <rdfs:comment xml:lang="en">Identifies the type of lineage being described, e.g., empowerment, instruction, reading transmission, etc.</rdfs:comment>
        <rdfs:label xml:lang="en">Lineage type</rdfs:label>
    </owl:Class>
    


    <!-- http://purl.bdrc.io/ontology/LogEntry -->

    <owl:Class rdf:about="http://purl.bdrc.io/ontology/LogEntry">
        <rdfs:subClassOf rdf:resource="http://purl.bdrc.io/ontology/Facet"/>
        <rdfs:comment xml:lang="en">Indicates who, what, and when an update to BDRC resources was made</rdfs:comment>
        <rdfs:label xml:lang="en">Log Entry</rdfs:label>
    </owl:Class>
    


    <!-- http://purl.bdrc.io/ontology/Note -->

    <owl:Class rdf:about="http://purl.bdrc.io/ontology/Note">
        <rdfs:subClassOf rdf:resource="http://purl.bdrc.io/ontology/Facet"/>
    </owl:Class>
    


    <!-- http://purl.bdrc.io/ontology/OutlineType -->

    <owl:Class rdf:about="http://purl.bdrc.io/ontology/OutlineType">
        <rdfs:subClassOf rdf:resource="http://purl.bdrc.io/ontology/Type"/>
    </owl:Class>
    


    <!-- http://purl.bdrc.io/ontology/PaginationType -->

    <owl:Class rdf:about="http://purl.bdrc.io/ontology/PaginationType">
        <rdfs:subClassOf rdf:resource="http://purl.bdrc.io/ontology/Type"/>
        <rdfs:comment xml:lang="en">Indicates whether the outlining is relative or absolute. This refers to the convention for WorkLocation information. Almost all outlining is done with absolute pagination.

Relative pagination uses pagination in the content of the work while absolute counts from the first image of a scanned volume an since there are 2 scanned pages of metadata in each volume, absolute pagination generally starts at 3.</rdfs:comment>
        <rdfs:comment xml:lang="en">Migration info: The pagination information affects the interpretation of the :WorkLocation(s) that occur in the original outline. The migration should add the pagination information to each WorkLocation since there will no longer be an Outline document</rdfs:comment>
        <rdfs:label xml:lang="en">pagination type</rdfs:label>
    </owl:Class>
    


    <!-- http://purl.bdrc.io/ontology/Person -->

    <owl:Class rdf:about="http://purl.bdrc.io/ontology/Person">
        <rdfs:subClassOf rdf:resource="http://purl.bdrc.io/ontology/Entity"/>
        <rdfs:comment rdf:datatype="http://www.w3.org/2001/XMLSchema#string">The Person object tracks biographical data such as kinship relations, birth and death dates, administrative offices  and seats held, important events and known name variants.  Instances of Person objects are not created for historical and quasi-historical personages, including legendary and mythical figures. Deities are defined as Topics.</rdfs:comment>
        <rdfs:comment xml:lang="en">names are represented via bdo:PersonName</rdfs:comment>
        <rdfs:label xml:lang="en">Person</rdfs:label>
    </owl:Class>
    


    <!-- http://purl.bdrc.io/ontology/PersonEvent -->

    <owl:Class rdf:about="http://purl.bdrc.io/ontology/PersonEvent">
        <rdfs:subClassOf rdf:resource="http://purl.bdrc.io/ontology/Facet"/>
        <rdfs:subClassOf>
            <owl:Restriction>
                <owl:onProperty rdf:resource="http://purl.bdrc.io/ontology/personEventCorporation"/>
                <owl:maxQualifiedCardinality rdf:datatype="http://www.w3.org/2001/XMLSchema#nonNegativeInteger">1</owl:maxQualifiedCardinality>
                <owl:onClass rdf:resource="http://purl.bdrc.io/ontology/Corporation"/>
            </owl:Restriction>
        </rdfs:subClassOf>
        <rdfs:subClassOf>
            <owl:Restriction>
                <owl:onProperty rdf:resource="http://purl.bdrc.io/ontology/personEventPlace"/>
                <owl:maxQualifiedCardinality rdf:datatype="http://www.w3.org/2001/XMLSchema#nonNegativeInteger">1</owl:maxQualifiedCardinality>
                <owl:onClass rdf:resource="http://purl.bdrc.io/ontology/Place"/>
            </owl:Restriction>
        </rdfs:subClassOf>
        <rdfs:subClassOf>
            <owl:Restriction>
                <owl:onProperty rdf:resource="http://purl.bdrc.io/ontology/personEventRole"/>
                <owl:maxQualifiedCardinality rdf:datatype="http://www.w3.org/2001/XMLSchema#nonNegativeInteger">1</owl:maxQualifiedCardinality>
                <owl:onClass rdf:resource="http://purl.bdrc.io/ontology/Role"/>
            </owl:Restriction>
        </rdfs:subClassOf>
        <inferSubTree rdf:datatype="http://www.w3.org/2001/XMLSchema#boolean">true</inferSubTree>
        <rdfs:comment xml:lang="en">The source person.xsd includes event/pid which is not used and should be silently discarded during migration.</rdfs:comment>
        <rdfs:label xml:lang="en">Person Event</rdfs:label>
    </owl:Class>
    


    <!-- http://purl.bdrc.io/ontology/PersonEventType -->

    <owl:Class rdf:about="http://purl.bdrc.io/ontology/PersonEventType">
        <rdfs:subClassOf rdf:resource="http://purl.bdrc.io/ontology/Type"/>
        <rdfs:comment xml:lang="en">For :PersonEvent(s) indicates the type of event, e.g., birth, death, marriage, final ordination, etc.</rdfs:comment>
        <rdfs:label xml:lang="en">Event</rdfs:label>
    </owl:Class>
    


    <!-- http://purl.bdrc.io/ontology/PersonIncarnationOf -->

    <owl:Class rdf:about="http://purl.bdrc.io/ontology/PersonIncarnationOf">
        <rdfs:subClassOf rdf:resource="http://purl.bdrc.io/ontology/Facet"/>
        <rdfs:comment>The IncarnationOf records which being (Person or Topic) this individual is an incarnation of and optionally what sort of incarnation (body speech, mind, etc). There are 1,456 individuals out of 18,320, that are marked as being incarnations of some being. Of these, 18 are marked with per:incarnationOf_relation and 5 are marked with per:incarnationOf_secondary.</rdfs:comment>
        <rdfs:label xml:lang="en">Incarnation of</rdfs:label>
    </owl:Class>
    


    <!-- http://purl.bdrc.io/ontology/PersonIncarnationType -->

    <owl:Class rdf:about="http://purl.bdrc.io/ontology/PersonIncarnationType">
        <rdfs:subClassOf rdf:resource="http://purl.bdrc.io/ontology/Type"/>
        <rdfs:comment xml:lang="en">Denotes the type of incarnation, e.g., general, body, speech, etc.</rdfs:comment>
        <rdfs:label xml:lang="en">Incarnation type</rdfs:label>
    </owl:Class>
    


    <!-- http://purl.bdrc.io/ontology/PersonName -->

    <owl:Class rdf:about="http://purl.bdrc.io/ontology/PersonName">
        <rdfs:subClassOf rdf:resource="http://purl.bdrc.io/ontology/Facet"/>
        <rdfs:comment xml:lang="en">represents a name of a Person via an rdfs:label and :personNameType :PersonNameType. For example:

    bdr:Pxxxx a :Person ;
               :personHasName [ a :PersonName ;
                                             rdfs:label &quot;dri med &apos;od zer&quot;@bo-x-ewts ;
                                             :personNameType bdr:PersonPrimaryName ]</rdfs:comment>
        <rdfs:label xml:lang="en">person name</rdfs:label>
    </owl:Class>
    


    <!-- http://purl.bdrc.io/ontology/PersonNameType -->

    <owl:Class rdf:about="http://purl.bdrc.io/ontology/PersonNameType">
        <rdfs:subClassOf rdf:resource="http://purl.bdrc.io/ontology/Type"/>
        <rdfs:comment xml:lang="en">Denotes the type of a :PersonName, e.g., first ordination, family, office title, etc.</rdfs:comment>
        <rdfs:label xml:lang="en">Name type</rdfs:label>
    </owl:Class>
    


    <!-- http://purl.bdrc.io/ontology/Place -->

    <owl:Class rdf:about="http://purl.bdrc.io/ontology/Place">
        <rdfs:subClassOf rdf:resource="http://purl.bdrc.io/ontology/Entity"/>
        <inferSubTree rdf:datatype="http://www.w3.org/2001/XMLSchema#boolean">true</inferSubTree>
        <rdfs:comment xml:lang="en">Names are represented by rdfs:label</rdfs:comment>
        <rdfs:comment xml:lang="en">Places are geographic entities ranging from monasteries, to villages, to counties, provinces and so on. Places are modeled in terms of subclasses that indicate the type of &quot;real world&quot; place that is referred to</rdfs:comment>
        <rdfs:label xml:lang="en">Place</rdfs:label>
    </owl:Class>
    


    <!-- http://purl.bdrc.io/ontology/PlaceAddress -->

    <owl:Class rdf:about="http://purl.bdrc.io/ontology/PlaceAddress">
        <rdfs:subClassOf rdf:resource="http://purl.bdrc.io/ontology/Facet"/>
        <rdfs:comment>The plc:Address allows to record conventional address informaton for a Place. It is added to support the Tibetan Library Management application that allows for recording holdings of Works from other libraries.</rdfs:comment>
    </owl:Class>
    


    <!-- http://purl.bdrc.io/ontology/PlaceEvent -->

    <owl:Class rdf:about="http://purl.bdrc.io/ontology/PlaceEvent">
        <rdfs:subClassOf rdf:resource="http://purl.bdrc.io/ontology/Facet"/>
        <inferSubTree rdf:datatype="http://www.w3.org/2001/XMLSchema#boolean">true</inferSubTree>
    </owl:Class>
    


    <!-- http://purl.bdrc.io/ontology/PlaceEventType -->

    <owl:Class rdf:about="http://purl.bdrc.io/ontology/PlaceEventType">
        <rdfs:subClassOf rdf:resource="http://purl.bdrc.io/ontology/Type"/>
        <rdfs:comment xml:lang="en">Place events record when, what, and who happened at a given :Place. The :PlaceEventType(s) denote the &quot;what&quot;, e.g., abandoned, converted, destroyed, etc.</rdfs:comment>
        <rdfs:label xml:lang="en">Place event type</rdfs:label>
    </owl:Class>
    


    <!-- http://purl.bdrc.io/ontology/PlaceType -->

    <owl:Class rdf:about="http://purl.bdrc.io/ontology/PlaceType">
        <rdfs:subClassOf rdf:resource="http://purl.bdrc.io/ontology/Type"/>
        <rdfs:comment xml:lang="en">The :PlaceType(s) are used to indicate a conventional characterization of a :Place, e.g., bdr:PlaceTypeBangSo, bdr:PlaceTypeChoBo, etc.</rdfs:comment>
        <rdfs:label xml:lang="en">Place Type</rdfs:label>
    </owl:Class>
    


    <!-- http://purl.bdrc.io/ontology/PrintType -->

    <owl:Class rdf:about="http://purl.bdrc.io/ontology/PrintType">
        <rdfs:subClassOf rdf:resource="http://purl.bdrc.io/ontology/Type"/>
        <rdfs:comment xml:lang="en">Type print: manuscript, computer, woodblock, etc.</rdfs:comment>
    </owl:Class>
    


    <!-- http://purl.bdrc.io/ontology/Role -->

    <owl:Class rdf:about="http://purl.bdrc.io/ontology/Role">
        <rdfs:subClassOf rdf:resource="http://purl.bdrc.io/ontology/Entity"/>
        <rdfs:comment xml:lang="en">Names are represented by rdfs:label</rdfs:comment>
        <rdfs:comment xml:lang="en">Roles include offices held as well as other positions. This was formerly called Office in the tbrc.org schema but is now using a terminology more commonly used in libraries.</rdfs:comment>
        <rdfs:label xml:lang="en">Role</rdfs:label>
    </owl:Class>
    


    <!-- http://purl.bdrc.io/ontology/StatusType -->

    <owl:Class rdf:about="http://purl.bdrc.io/ontology/StatusType">
        <rdfs:subClassOf rdf:resource="http://purl.bdrc.io/ontology/Type"/>
    </owl:Class>
    


    <!-- http://purl.bdrc.io/ontology/Taxonomy -->

    <owl:Class rdf:about="http://purl.bdrc.io/ontology/Taxonomy">
        <rdfs:subClassOf rdf:resource="http://purl.bdrc.io/ontology/Entity"/>
        <rdfs:comment xml:lang="en">A :Taxonomy individual represents a hierarchical organization of a collection of individuals - usually instances of a subclass of :Type. For example, the individuals of type :KinType are organized via the bdr:KinshipTaxonomy.

Assertions using :taxSubClass and :taxElementOf object properties organize the set of typed individuals into a class/subclass hierarchy. Typed indivduals can be asserted to be :taxSubClass of other individuals or of the :Taxonomy individual itself - the :Taxonomy individual is the root of the class/subclass hierarchy.

Typed individuals are asserted to be :taxElementOf other typed individuals that are :taxSubClass related to the :Taxonomy individual.

This approach allows for typed individuals to be elements or subclass as needed for the given taxonomy. For example, 

    :KinType owl:subClassOf :Type .

    bdr:KinshipTaxonomy a :Taxonomy .

    bdr:KinParentSibling a :KinType ;
                                     :taxSubClass bdr:KinshipTaxonomy

    bdr:KinUncle a :KinType ;
                         :taxSubClass bdr:KinParentSibling

and

    bdr:KinPaternalUncle a :KinType ;
    bdr:KinPaternalUncle :taxElementOf bdr:KinUncle .

permits one to assert that

    bdr:Pxxxx [ a :Kin ;
                       :personKinType bdr:KinUncle ;
                       :personKinWho bdr:Pyyyy ]

or if there is more specificity known:


    bdr:Pxxxx [ a :Kin ;
                       :personKinType bdr:KinPaternalUncle ;
                       :personKinWho bdr:Pyyyy ]

The idea of distinguishing :taxElementOf versus :taxSubClass allows to indicate what can be extended and what typed individuals are &quot;final&quot;.

If all typed individuals represent extendable entities then they can all be asserted as :taxSubClass.

Using typed individuals provides a straightforward approach to localization by simply attaching rdfs:label in the various languages to eah of the typed individuals so that bdr:KinUncle will have the zh, bo, and en labels needed to display in an application.

Using typed individuals allows to provide a uniform approach to typing names, events, groups and so on rather than using owl:class/subclass relations in some cases and sub-properties (data or object) in other cases.</rdfs:comment>
        <rdfs:comment xml:lang="en">Rules should be added to indicate that :taxElementOf and :taxSubClass should be used with a &quot;coherent&quot; set of individuals of type :Type. In other words the set of individuals related among themselves and a :Taxonomy individual should be all of the same :Type (or maybe family of types).

Futher there should be inference rules for :taxElementOf and :taxSubClass so that queries for bdr:KinUncle find also instances of bdr:PaternalUncle and so on.</rdfs:comment>
        <rdfs:comment xml:lang="en">Support for multiple Taxonomies organizing the same set of inidividuals is provided by using the properties :taxSubclassProperty and :taxElementOfProperty:

bdr:KinshipTaxonomy a :Taxonomy ;
      :taxSubclassProperty :taxSubclass ;
      :taxElementOfProperty :taxElementOf .

If there were an alternative Taxonomy, bdr:OtherTaxonomy:

bdr:OtherTaxonomy a :Taxonomy ;
      :taxSubclassProperty :taxSubclass02 ;
      :taxElementOfProperty :taxElementOf02 .

Would allow for bdr:OtherTaxonomy to organize the same set of Kinship individuals unambiguously.</rdfs:comment>
        <rdfs:label xml:lang="en">Taxonomy</rdfs:label>
    </owl:Class>
    


    <!-- http://purl.bdrc.io/ontology/Topic -->

    <owl:Class rdf:about="http://purl.bdrc.io/ontology/Topic">
        <rdfs:subClassOf rdf:resource="http://purl.bdrc.io/ontology/Entity"/>
        <rdfs:comment xml:lang="en">Names are represented by rdfs:label</rdfs:comment>
        <rdfs:comment>Subjects Just as in a traditional library catalog, each Work in the knowledgebase can be classified under one or more Subject Headings. A Subject Heading can be one of the following things: 1. A technical term; 2. The title of a Work; 3. The name of a Person; 4. The name of a Place. A technical term (e.g. mandala or sgrub thabs can have any number of Equivalent Meanings from other languages. The other types of Subject Headings (Work Titles, Person Names, Place Names) are also Library Objects with their own records in the Works, Persons, or Places databases. Each Subject Headings record is composed of several fields. Not every field appears in each record. Click on the links below for more information about these fields. Subtopics: Subject Headings that are connected to Works Subject Headings with equivalent meanings Subject Headings Usage Information See also: Library Objects | Subject Search</rdfs:comment>
        <rdfs:comment>The topic.xsd &lt;seeAlso/&gt; is model via the top:seeAlso annotation property</rdfs:comment>
        <rdfs:label xml:lang="en">Topic</rdfs:label>
    </owl:Class>
    


    <!-- http://purl.bdrc.io/ontology/Tradition -->

    <owl:Class rdf:about="http://purl.bdrc.io/ontology/Tradition">
        <rdfs:subClassOf rdf:resource="http://purl.bdrc.io/ontology/Type"/>
        <rdfs:comment xml:lang="en">Individuals represent various (Tibetan) Buddhist traditions</rdfs:comment>
        <rdfs:label xml:lang="en">Tradition</rdfs:label>
    </owl:Class>
    


    <!-- http://purl.bdrc.io/ontology/Type -->

    <owl:Class rdf:about="http://purl.bdrc.io/ontology/Type">
        <rdfs:comment xml:lang="en">Types are used to indicate features names, titles, events and so on.

An owl:subClassOf :Type, e.g., :KinType, will have some set of individuals that represent the various types, e.g., bdr:KinUncle, bdr:KinYoungerSister, etc.

The set of such individuals may be further organized via :Taxonomy but need not be.</rdfs:comment>
        <rdfs:label xml:lang="en">Type</rdfs:label>
    </owl:Class>
    


    <!-- http://purl.bdrc.io/ontology/Volume -->

    <owl:Class rdf:about="http://purl.bdrc.io/ontology/Volume">
        <rdfs:subClassOf rdf:resource="http://purl.bdrc.io/ontology/Facet"/>
        <rdfs:comment>Each vol:Volume MAY have a desc:onDisk property which will have a &apos;|&apos; separated list of names of the page image files. This property is present when the subject volume has been digitized and deposited in the online archive. Otherwise, the volume will have properties related to the total number of pages, intro pages and so on as well as relevant information from the originating ScanRequest.</rdfs:comment>
    </owl:Class>
    


    <!-- http://purl.bdrc.io/ontology/Work -->

    <owl:Class rdf:about="http://purl.bdrc.io/ontology/Work">
        <rdfs:subClassOf rdf:resource="http://purl.bdrc.io/ontology/Entity"/>
        <rdfs:comment xml:lang="en">NB: The definition of &lt;w:info/&gt; in work.xsd is incorrect since it allows unbounded use of &lt;w:info/&gt;. It should have been spec&apos;d as only 1 occurrence. Hence in the ontology the wrk:info properties have domain wrk:Work rather than introducing an anon class</rdfs:comment>
        <rdfs:comment xml:lang="en">Note that &lt;archiveInfo/&gt; @distribution and @restriction are not used and not migrated. They have been replaced by @license and access.</rdfs:comment>
        <rdfs:comment xml:lang="en">The wrk:Work resource models the descriptive metadata about a &quot;book&quot; in the BUDAverse. The legacy model split the descriptive metadata between Works and Pubinfos ( predominantly publication data). Thisr ontology merges the Work and Pubinfo items under the wrk:Work resource so there is no hasPubinfo property.

The Works also included some structural metadata in the volumeMap but that is moved to the vol:Volumes resource in this ontology.</rdfs:comment>
        <rdfs:label xml:lang="en">Work</rdfs:label>
    </owl:Class>
    


    <!-- http://purl.bdrc.io/ontology/WorkAccessType -->

    <owl:Class rdf:about="http://purl.bdrc.io/ontology/WorkAccessType">
        <rdfs:subClassOf rdf:resource="http://purl.bdrc.io/ontology/Type"/>
        <rdfs:comment xml:lang="en">The type of access reflects whether and how much of the content of a Work is made available online.</rdfs:comment>
        <rdfs:label xml:lang="en">Work Access Type</rdfs:label>
    </owl:Class>
    


    <!-- http://purl.bdrc.io/ontology/WorkCreator -->

    <owl:Class rdf:about="http://purl.bdrc.io/ontology/WorkCreator">
        <rdfs:subClassOf rdf:resource="http://purl.bdrc.io/ontology/Facet"/>
    </owl:Class>
    


    <!-- http://purl.bdrc.io/ontology/WorkCreatorType -->

    <owl:Class rdf:about="http://purl.bdrc.io/ontology/WorkCreatorType">
        <rdfs:subClassOf rdf:resource="http://purl.bdrc.io/ontology/Type"/>
    </owl:Class>
    


    <!-- http://purl.bdrc.io/ontology/WorkHolding -->

    <owl:Class rdf:about="http://purl.bdrc.io/ontology/WorkHolding">
        <rdfs:subClassOf rdf:resource="http://purl.bdrc.io/ontology/Facet"/>
        <rdfs:comment xml:lang="en">A holding refers to the library Place which has one or more physical copies of the  catalogued Work and shows the number of copies that are held at the library. The CData for the Holding is the Library&apos;s shelving information concerning the location in the library of the physical copies. The exception is an optional note regarding missing volumes in a copy or other information such as may  be useful to qualify the status of one or more copies.

Example:

bdr:W1TLMTGA000883 a :Work ;
      :workHasHolding [ a :WorkHolding ;
            :workHoldingLibrary bdr:G1TLMTGA000001 ;
            :workHoldingCopies 1 ;
            :workHoldingShelf &quot;ཇ|ཇ|༣||001278&quot; ;
            :workHoldingCode &quot;TGA&quot; ] ;
      :workHasHolding [ a :WorkHolding ;
            :workHoldingLibrary bdr:G1TLMTGB000001 ;
            :workHoldingCopies 1 ;
            :workHoldingShelf &quot;ག|༦|||000026&quot; ;
            :workHoldingCode &quot;TGB&quot; ] .

bdr:W20907 a :Work ;
      :workHasHolding [ a :WorkHolding ;
            :workHoldingLibrary bdr:G1TLMTGA000001 ;
            :workHoldingCopies 1 ;
            :workHoldingShelf &quot;&gt;ཉ|༣|||000567&quot; ;
            :workHoldingCode &quot;TGA&quot; ] .

bdr:W1KG20928 a :Work ;
      :workHasHolding [ a :WorkHolding ;
            :workHoldingLibrary bdr:G1TLMTGA000001 ;
            :workHoldingCopies 1 ;
            :workHoldingShelf &quot;&gt;ཉ|༣|||001811&quot; ;
            :workHoldingCode &quot;TGA&quot; ] ;
            :workHoldingException &quot;དེབ་གཅིག་ཕྱི་ལ་གཡར་ནས་མ་འབྱོར&quot;@bo .</rdfs:comment>
        <rdfs:label xml:lang="en">Holding</rdfs:label>
    </owl:Class>
    


    <!-- http://purl.bdrc.io/ontology/WorkLicense -->

    <owl:Class rdf:about="http://purl.bdrc.io/ontology/WorkLicense">
        <rdfs:subClassOf rdf:resource="http://purl.bdrc.io/ontology/Type"/>
        <rdfs:comment xml:lang="en">The license under which access to the Work is provided</rdfs:comment>
        <rdfs:label xml:lang="en">License</rdfs:label>
    </owl:Class>
    


    <!-- http://purl.bdrc.io/ontology/WorkLocation -->

    <owl:Class rdf:about="http://purl.bdrc.io/ontology/WorkLocation">
        <rdfs:subClassOf rdf:resource="http://purl.bdrc.io/ontology/Facet"/>
        <inferSubTree rdf:datatype="http://www.w3.org/2001/XMLSchema#boolean">true</inferSubTree>
        <rdfs:comment xml:lang="en">The WorkLocation describes the Work, Volume, Page and so on at which something of interest occurs, e.g., the beginning or end of a Work that is contained in another Work; or a reference to the source of a Lineage</rdfs:comment>
        <rdfs:comment>The following explains the intent of splitting an Outline into chunks when outlining very large works. This is why there is a &lt;o:location/&gt; element spec&apos;d in the outline.xsd; however, this feature has not been used in this manner but rather as a redundant marker of which work is being outlined. In the case that the Outline is the detail of a particular Text then the location typically will specify the Work and Volume (relative to 1) that contains the Outlined Text. Thus Locations on the sub-structure need only mention page, line and phrase</rdfs:comment>
        <rdfs:comment>parent facet of Work locations by page and folio. The XSD defn is located in common.xsd but is move to Work in the new ontology since that is a more appropriate location</rdfs:comment>
    </owl:Class>
    


    <!-- http://purl.bdrc.io/ontology/WorkLocationType -->

    <owl:Class rdf:about="http://purl.bdrc.io/ontology/WorkLocationType">
        <rdfs:subClassOf rdf:resource="http://purl.bdrc.io/ontology/Type"/>
        <rdfs:comment xml:lang="en">Indicates whether the WorkLocation is the beginning or end of a reference into a Work. An untyped WorkLocation may include a :workLocationFF indicating the number of following pages. This won&apos;t always work when the reference spans volumes as with some of the very long texts in Kanjur</rdfs:comment>
        <rdfs:label xml:lang="en">Work Location Type</rdfs:label>
    </owl:Class>
    


    <!-- http://purl.bdrc.io/ontology/WorkPartType -->

    <owl:Class rdf:about="http://purl.bdrc.io/ontology/WorkPartType">
        <rdfs:subClassOf rdf:resource="http://purl.bdrc.io/ontology/Type"/>
    </owl:Class>
    


    <!-- http://purl.bdrc.io/ontology/WorkPubinfoSeries -->

    <owl:Class rdf:about="http://purl.bdrc.io/ontology/WorkPubinfoSeries">
        <rdfs:subClassOf rdf:resource="http://purl.bdrc.io/ontology/Facet"/>
    </owl:Class>
    


    <!-- http://purl.bdrc.io/ontology/WorkRefs -->

    <owl:Class rdf:about="http://purl.bdrc.io/ontology/WorkRefs">
        <rdfs:subClassOf rdf:resource="http://purl.bdrc.io/ontology/Facet"/>
        <rdfs:comment xml:lang="en">Blank nodes of this class collect together the various reference numbers that apply to a given work. This is primarily used in Kanjurs and Tengyurs for which there are quite a number of different catalogue number schemes.</rdfs:comment>
        <rdfs:label xml:lang="en">Work References</rdfs:label>
        <rdfs:seeAlso rdf:resource="https://www.istb.univie.ac.at/kanjur/xml4/sub/sigla.php"/>
    </owl:Class>
    


    <!-- http://purl.bdrc.io/ontology/WorkSite -->

    <owl:Class rdf:about="http://purl.bdrc.io/ontology/WorkSite">
        <rdfs:subClassOf rdf:resource="http://purl.bdrc.io/ontology/Facet"/>
        <inferSubTree rdf:datatype="http://www.w3.org/2001/XMLSchema#boolean">true</inferSubTree>
    </owl:Class>
    


    <!-- http://purl.bdrc.io/ontology/WorkSiteType -->

    <owl:Class rdf:about="http://purl.bdrc.io/ontology/WorkSiteType">
        <rdfs:subClassOf rdf:resource="http://purl.bdrc.io/ontology/Type"/>
        <rdfs:comment xml:lang="en">Indicates what type of activity, e.g., completed, edited, printed, etc., regarding a work occurred at some site (:WorkSite)</rdfs:comment>
        <rdfs:label xml:lang="en">Site what</rdfs:label>
    </owl:Class>
    


    <!-- http://purl.bdrc.io/ontology/WorkTitle -->

    <owl:Class rdf:about="http://purl.bdrc.io/ontology/WorkTitle">
        <rdfs:subClassOf rdf:resource="http://purl.bdrc.io/ontology/Facet"/>
        <rdfs:comment xml:lang="en">A title for the Work including the title text and title type: full, sub, etc:


bdr:W22083 a :Work ;
      :workHasTitle [ a :WorkTitle ;
            :workTitleType bdr:WorkBibliogrpahicTitle ;
            rdfs:label &quot;bka&apos; &apos;gyur (stog pho brang bris ma/)&quot;@bo-x-ewts ] ;
      :workHasTitle [ a :WorkTitle ;
            :workTitleType bdr:WorkOtherTitle ;
            rdfs:label &quot;la dwags tog mu mkhar bzhugs pa&apos;i bod yig bka&apos; &apos;gyur bris ma/&quot;@bo-x-ewts ] ;
      :workHasTitle [ a :WorkTitle ;
            :workTitleType bdr:WorkTitlePageTitle ;
            rdfs:label &quot;the tog palace manuscript of the tibetan kanjur&quot;@en ] .</rdfs:comment>
        <rdfs:label xml:lang="en">Title</rdfs:label>
    </owl:Class>
    


    <!-- http://purl.bdrc.io/ontology/WorkTitleType -->

    <owl:Class rdf:about="http://purl.bdrc.io/ontology/WorkTitleType">
        <rdfs:subClassOf rdf:resource="http://purl.bdrc.io/ontology/Type"/>
    </owl:Class>
    


    <!-- http://purl.bdrc.io/ontology/WorkType -->

    <owl:Class rdf:about="http://purl.bdrc.io/ontology/WorkType">
        <rdfs:subClassOf rdf:resource="http://purl.bdrc.io/ontology/Type"/>
        <rdfs:comment xml:lang="en">The type of Work - from legacy metadata: publishedWork, unicodeText, etc. This is from the &lt;work:info @nodeType/&gt;</rdfs:comment>
        <rdfs:label xml:lang="en">type of work</rdfs:label>
    </owl:Class>
    


    <!-- http://purl.bdrc.io/ontology/admin/Admin -->

    <owl:Class rdf:about="http://purl.bdrc.io/ontology/admin/Admin"/>
    


    <!-- http://purl.bdrc.io/ontology/admin/LogEntry -->

    <owl:Class rdf:about="http://purl.bdrc.io/ontology/admin/LogEntry">
        <rdfs:subClassOf rdf:resource="http://purl.bdrc.io/ontology/admin/Admin"/>
        <rdfs:comment xml:lang="en">Log entries for :Entity updates. Includes the agent, date and message explaing the update.</rdfs:comment>
        <rdfs:label xml:lang="en">Log Entry</rdfs:label>
    </owl:Class>
    


    <!-- http://purl.bdrc.io/ontology/admin/Product -->

    <owl:Class rdf:about="http://purl.bdrc.io/ontology/admin/Product">
        <rdfs:subClassOf rdf:resource="http://purl.bdrc.io/ontology/admin/Admin"/>
        <rdfs:comment>An Product represents a collection of works that are distributed together. Historically this has meant on a CDROM, DVDROM or harddrive; nowadays, Products are used mostly to collect Works that are made available to institutional subscribers online via IP-address validation. Although there are still harddrive collections prepared from Products.

IP-address validation is supported by adding to a Product sets of address ranges organized by organizations, like UCB, TUMS etc. When the migration ontology is normalized these sets of address ranges should be given their own resource outside of the Product resource since the model of institutional subscriptions is being changed so that it is not Product centric.

Products have decs:contents rather than a :name (but this can be added during normalization). 

The various Works that are contained in the Product include an inProduct element that refers back to the Product. So to find all the Works that are contained in a Product is a simple query. to locate all Works that refer to a given Product via wrk:inProduct.</rdfs:comment>
        <rdfs:comment xml:lang="en">Names are represented by rdfs:label</rdfs:comment>
        <rdfs:label xml:lang="en">Product</rdfs:label>
    </owl:Class>
    


    <!-- http://purl.bdrc.io/ontology/admin/ProductOrg -->

    <owl:Class rdf:about="http://purl.bdrc.io/ontology/admin/ProductOrg">
        <rdfs:subClassOf rdf:resource="http://purl.bdrc.io/ontology/admin/Admin"/>
        <rdfs:comment xml:lang="en">A ProductOrg is a unit of organization for IP-address based access control, e.g., the University of California System, PR99UCS01. A ProductOrg may have zero or more ProductOrg members, via productHasOrg, to allow for organizing large multi-level organizations such as the U. California system. Also a ProductOrg may have zero or more productHasAllow assertions to indicate IP address ranges that are allowed access.</rdfs:comment>
        <rdfs:comment xml:lang="en">the name of a ProductOrg is represented by rdfs:label</rdfs:comment>
    </owl:Class>
    


    <!-- http://www.w3.org/2002/07/owl#Thing -->

    <rdf:Description rdf:about="http://www.w3.org/2002/07/owl#Thing">
        <rdfs:comment xml:lang="en">the set of all Things in the bdrc ontology are factored into subsets that represent 

    the principle concepts/entities
    facets/n-ary properties of the principle concepts
    types of resources such as place events, work titles and so on 
    classes from 3rd party ontologies that are referred to</rdfs:comment>
    </rdf:Description>
    


    <!-- http://xmlns.com/foaf/0.1/Agent -->

    <owl:Class rdf:about="http://xmlns.com/foaf/0.1/Agent"/>
    


    <!-- 
    ///////////////////////////////////////////////////////////////////////////////////////
    //
    // Individuals
    //
    ///////////////////////////////////////////////////////////////////////////////////////
     -->

    


    <!-- http://purl.bdrc.io/resource/CorporationMemberTypeByBlood -->

    <owl:NamedIndividual rdf:about="http://purl.bdrc.io/resource/CorporationMemberTypeByBlood">
        <rdf:type rdf:resource="http://purl.bdrc.io/ontology/CorporationMemberType"/>
    </owl:NamedIndividual>
    


    <!-- http://purl.bdrc.io/resource/CorporationMemberTypeByMarriage -->

    <owl:NamedIndividual rdf:about="http://purl.bdrc.io/resource/CorporationMemberTypeByMarriage">
        <rdf:type rdf:resource="http://purl.bdrc.io/ontology/CorporationMemberType"/>
    </owl:NamedIndividual>
    


    <!-- http://purl.bdrc.io/resource/CorporationMemberTypeMonastic -->

    <owl:NamedIndividual rdf:about="http://purl.bdrc.io/resource/CorporationMemberTypeMonastic">
        <rdf:type rdf:resource="http://purl.bdrc.io/ontology/CorporationMemberType"/>
    </owl:NamedIndividual>
    


    <!-- http://purl.bdrc.io/resource/CorporationMemberTypeNotSpecified -->

    <owl:NamedIndividual rdf:about="http://purl.bdrc.io/resource/CorporationMemberTypeNotSpecified">
        <rdf:type rdf:resource="http://purl.bdrc.io/ontology/CorporationMemberType"/>
    </owl:NamedIndividual>
    


    <!-- http://purl.bdrc.io/resource/CreatorTypeArtist -->

    <owl:NamedIndividual rdf:about="http://purl.bdrc.io/resource/CreatorTypeArtist">
        <rdf:type rdf:resource="http://purl.bdrc.io/ontology/WorkCreatorType"/>
    </owl:NamedIndividual>
    


    <!-- http://purl.bdrc.io/resource/CreatorTypeAttributedAuthor -->

    <owl:NamedIndividual rdf:about="http://purl.bdrc.io/resource/CreatorTypeAttributedAuthor">
        <rdf:type rdf:resource="http://purl.bdrc.io/ontology/WorkCreatorType"/>
    </owl:NamedIndividual>
    


    <!-- http://purl.bdrc.io/resource/CreatorTypeBard -->

    <owl:NamedIndividual rdf:about="http://purl.bdrc.io/resource/CreatorTypeBard">
        <rdf:type rdf:resource="http://purl.bdrc.io/ontology/WorkCreatorType"/>
    </owl:NamedIndividual>
    


    <!-- http://purl.bdrc.io/resource/CreatorTypeCalligrapher -->

    <owl:NamedIndividual rdf:about="http://purl.bdrc.io/resource/CreatorTypeCalligrapher">
        <rdf:type rdf:resource="http://purl.bdrc.io/ontology/WorkCreatorType"/>
    </owl:NamedIndividual>
    


    <!-- http://purl.bdrc.io/resource/CreatorTypeCommentator -->

    <owl:NamedIndividual rdf:about="http://purl.bdrc.io/resource/CreatorTypeCommentator">
        <rdf:type rdf:resource="http://purl.bdrc.io/ontology/WorkCreatorType"/>
    </owl:NamedIndividual>
    


    <!-- http://purl.bdrc.io/resource/CreatorTypeContributingAuthor -->

    <owl:NamedIndividual rdf:about="http://purl.bdrc.io/resource/CreatorTypeContributingAuthor">
        <rdf:type rdf:resource="http://purl.bdrc.io/ontology/WorkCreatorType"/>
    </owl:NamedIndividual>
    


    <!-- http://purl.bdrc.io/resource/CreatorTypeEditor -->

    <owl:NamedIndividual rdf:about="http://purl.bdrc.io/resource/CreatorTypeEditor">
        <rdf:type rdf:resource="http://purl.bdrc.io/ontology/WorkCreatorType"/>
    </owl:NamedIndividual>
    


    <!-- http://purl.bdrc.io/resource/CreatorTypeGeneralAuthor -->

    <owl:NamedIndividual rdf:about="http://purl.bdrc.io/resource/CreatorTypeGeneralAuthor">
        <rdf:type rdf:resource="http://purl.bdrc.io/ontology/WorkCreatorType"/>
    </owl:NamedIndividual>
    


    <!-- http://purl.bdrc.io/resource/CreatorTypeMainAuthor -->

    <owl:NamedIndividual rdf:about="http://purl.bdrc.io/resource/CreatorTypeMainAuthor">
        <rdf:type rdf:resource="http://purl.bdrc.io/ontology/WorkCreatorType"/>
    </owl:NamedIndividual>
    


    <!-- http://purl.bdrc.io/resource/CreatorTypePandita -->

    <owl:NamedIndividual rdf:about="http://purl.bdrc.io/resource/CreatorTypePandita">
        <rdf:type rdf:resource="http://purl.bdrc.io/ontology/WorkCreatorType"/>
    </owl:NamedIndividual>
    


    <!-- http://purl.bdrc.io/resource/CreatorTypeRecipientOfResponseToQuery -->

    <owl:NamedIndividual rdf:about="http://purl.bdrc.io/resource/CreatorTypeRecipientOfResponseToQuery">
        <rdf:type rdf:resource="http://purl.bdrc.io/ontology/WorkCreatorType"/>
    </owl:NamedIndividual>
    


    <!-- http://purl.bdrc.io/resource/CreatorTypeRequester -->

    <owl:NamedIndividual rdf:about="http://purl.bdrc.io/resource/CreatorTypeRequester">
        <rdf:type rdf:resource="http://purl.bdrc.io/ontology/WorkCreatorType"/>
    </owl:NamedIndividual>
    


    <!-- http://purl.bdrc.io/resource/CreatorTypeReviserOfTranslation -->

    <owl:NamedIndividual rdf:about="http://purl.bdrc.io/resource/CreatorTypeReviserOfTranslation">
        <rdf:type rdf:resource="http://purl.bdrc.io/ontology/WorkCreatorType"/>
    </owl:NamedIndividual>
    


    <!-- http://purl.bdrc.io/resource/CreatorTypeScribe -->

    <owl:NamedIndividual rdf:about="http://purl.bdrc.io/resource/CreatorTypeScribe">
        <rdf:type rdf:resource="http://purl.bdrc.io/ontology/WorkCreatorType"/>
    </owl:NamedIndividual>
    


    <!-- http://purl.bdrc.io/resource/CreatorTypeTerton -->

    <owl:NamedIndividual rdf:about="http://purl.bdrc.io/resource/CreatorTypeTerton">
        <rdf:type rdf:resource="http://purl.bdrc.io/ontology/WorkCreatorType"/>
    </owl:NamedIndividual>
    


    <!-- http://purl.bdrc.io/resource/CreatorTypeTranslator -->

    <owl:NamedIndividual rdf:about="http://purl.bdrc.io/resource/CreatorTypeTranslator">
        <rdf:type rdf:resource="http://purl.bdrc.io/ontology/WorkCreatorType"/>
    </owl:NamedIndividual>
    


    <!-- http://purl.bdrc.io/resource/GenderFemale -->

    <owl:NamedIndividual rdf:about="http://purl.bdrc.io/resource/GenderFemale">
        <rdf:type rdf:resource="http://purl.bdrc.io/ontology/Gender"/>
    </owl:NamedIndividual>
    


    <!-- http://purl.bdrc.io/resource/GenderMale -->

    <owl:NamedIndividual rdf:about="http://purl.bdrc.io/resource/GenderMale">
        <rdf:type rdf:resource="http://purl.bdrc.io/ontology/Gender"/>
    </owl:NamedIndividual>
    


    <!-- http://purl.bdrc.io/resource/GenderNotSpecified -->

    <owl:NamedIndividual rdf:about="http://purl.bdrc.io/resource/GenderNotSpecified">
        <rdf:type rdf:resource="http://purl.bdrc.io/ontology/Gender"/>
    </owl:NamedIndividual>
    


    <!-- http://purl.bdrc.io/resource/IncarnationTypeActivities -->

    <owl:NamedIndividual rdf:about="http://purl.bdrc.io/resource/IncarnationTypeActivities">
        <rdf:type rdf:resource="http://purl.bdrc.io/ontology/PersonIncarnationType"/>
        <rdfs:label xml:lang="en">activities incarnation</rdfs:label>
    </owl:NamedIndividual>
    


    <!-- http://purl.bdrc.io/resource/IncarnationTypeBody -->

    <owl:NamedIndividual rdf:about="http://purl.bdrc.io/resource/IncarnationTypeBody">
        <rdf:type rdf:resource="http://purl.bdrc.io/ontology/PersonIncarnationType"/>
        <rdfs:label xml:lang="en">body incarnation</rdfs:label>
    </owl:NamedIndividual>
    


    <!-- http://purl.bdrc.io/resource/IncarnationTypeGeneral -->

    <owl:NamedIndividual rdf:about="http://purl.bdrc.io/resource/IncarnationTypeGeneral">
        <rdf:type rdf:resource="http://purl.bdrc.io/ontology/PersonIncarnationType"/>
        <rdfs:label xml:lang="en">general incarnation</rdfs:label>
    </owl:NamedIndividual>
    


    <!-- http://purl.bdrc.io/resource/IncarnationTypeMind -->

    <owl:NamedIndividual rdf:about="http://purl.bdrc.io/resource/IncarnationTypeMind">
        <rdf:type rdf:resource="http://purl.bdrc.io/ontology/PersonIncarnationType"/>
        <rdfs:label xml:lang="en">mind incarnation</rdfs:label>
    </owl:NamedIndividual>
    


    <!-- http://purl.bdrc.io/resource/IncarnationTypeQualities -->

    <owl:NamedIndividual rdf:about="http://purl.bdrc.io/resource/IncarnationTypeQualities">
        <rdf:type rdf:resource="http://purl.bdrc.io/ontology/PersonIncarnationType"/>
        <rdfs:label xml:lang="en">qualities incarnation</rdfs:label>
    </owl:NamedIndividual>
    


    <!-- http://purl.bdrc.io/resource/IncarnationTypeSpeech -->

    <owl:NamedIndividual rdf:about="http://purl.bdrc.io/resource/IncarnationTypeSpeech">
        <rdf:type rdf:resource="http://purl.bdrc.io/ontology/PersonIncarnationType"/>
        <rdfs:label xml:lang="en">speech incarnation</rdfs:label>
    </owl:NamedIndividual>
    


    <!-- http://purl.bdrc.io/resource/IncarnationTypeYangtse -->

    <owl:NamedIndividual rdf:about="http://purl.bdrc.io/resource/IncarnationTypeYangtse">
        <rdf:type rdf:resource="http://purl.bdrc.io/ontology/PersonIncarnationType"/>
        <rdfs:label xml:lang="en">yangtse</rdfs:label>
    </owl:NamedIndividual>
    


    <!-- http://purl.bdrc.io/resource/ItemTypeEtextInput -->

    <owl:NamedIndividual rdf:about="http://purl.bdrc.io/resource/ItemTypeEtextInput">
        <rdf:type rdf:resource="http://purl.bdrc.io/ontology/ItemType"/>
        <rdfs:comment xml:lang="en">An eText created by human input of a text rather than OCR</rdfs:comment>
        <rdfs:label xml:lang="en">Input eText</rdfs:label>
    </owl:NamedIndividual>
    


    <!-- http://purl.bdrc.io/resource/ItemTypeImageAsset -->

    <owl:NamedIndividual rdf:about="http://purl.bdrc.io/resource/ItemTypeImageAsset">
        <rdf:type rdf:resource="http://purl.bdrc.io/ontology/ItemType"/>
        <rdfs:comment xml:lang="en">A collection of images, scanned, captured with camera, or microfilm conversion that comprise one or more volumes of a :Work</rdfs:comment>
        <rdfs:label xml:lang="en">Image Asset</rdfs:label>
    </owl:NamedIndividual>
    


    <!-- http://purl.bdrc.io/resource/ItemTypeOCREtext -->

    <owl:NamedIndividual rdf:about="http://purl.bdrc.io/resource/ItemTypeOCREtext">
        <rdf:type rdf:resource="http://purl.bdrc.io/ontology/ItemType"/>
        <rdfs:comment xml:lang="en">An eText created by OCR of an Image Asset. This is relevant since OCR&apos;d items allow for matching eText content to the original image.</rdfs:comment>
        <rdfs:label xml:lang="en">OCR&apos;d eText</rdfs:label>
    </owl:NamedIndividual>
    


    <!-- http://purl.bdrc.io/resource/ItemTypePhysicalHolding -->

    <owl:NamedIndividual rdf:about="http://purl.bdrc.io/resource/ItemTypePhysicalHolding">
        <rdf:type rdf:resource="http://purl.bdrc.io/ontology/ItemType"/>
        <rdfs:comment xml:lang="en">A physical holding in a particular library (Place)</rdfs:comment>
        <rdfs:label xml:lang="en">Physical Holding</rdfs:label>
    </owl:NamedIndividual>
    


    <!-- http://purl.bdrc.io/resource/KinAunt -->

    <owl:NamedIndividual rdf:about="http://purl.bdrc.io/resource/KinAunt">
        <rdf:type rdf:resource="http://purl.bdrc.io/ontology/KinType"/>
        <taxSubClass rdf:resource="http://purl.bdrc.io/resource/KinParentSibling"/>
    </owl:NamedIndividual>
    


    <!-- http://purl.bdrc.io/resource/KinBrother -->

    <owl:NamedIndividual rdf:about="http://purl.bdrc.io/resource/KinBrother">
        <rdf:type rdf:resource="http://purl.bdrc.io/ontology/KinType"/>
        <taxSubClass rdf:resource="http://purl.bdrc.io/resource/KinSibling"/>
    </owl:NamedIndividual>
    


    <!-- http://purl.bdrc.io/resource/KinChild -->

    <owl:NamedIndividual rdf:about="http://purl.bdrc.io/resource/KinChild">
        <rdf:type rdf:resource="http://purl.bdrc.io/ontology/KinType"/>
        <taxSubClass rdf:resource="http://purl.bdrc.io/resource/KinshipTaxonomy"/>
    </owl:NamedIndividual>
    


    <!-- http://purl.bdrc.io/resource/KinCousin -->

    <owl:NamedIndividual rdf:about="http://purl.bdrc.io/resource/KinCousin">
        <rdf:type rdf:resource="http://purl.bdrc.io/ontology/KinType"/>
        <taxSubClass rdf:resource="http://purl.bdrc.io/resource/KinshipTaxonomy"/>
    </owl:NamedIndividual>
    


    <!-- http://purl.bdrc.io/resource/KinDaughter -->

    <owl:NamedIndividual rdf:about="http://purl.bdrc.io/resource/KinDaughter">
        <rdf:type rdf:resource="http://purl.bdrc.io/ontology/KinType"/>
        <taxElementOf rdf:resource="http://purl.bdrc.io/resource/KinChild"/>
    </owl:NamedIndividual>
    


    <!-- http://purl.bdrc.io/resource/KinDaughterInLaw -->

    <owl:NamedIndividual rdf:about="http://purl.bdrc.io/resource/KinDaughterInLaw">
        <rdf:type rdf:resource="http://purl.bdrc.io/ontology/KinType"/>
        <taxElementOf rdf:resource="http://purl.bdrc.io/resource/KinInLaw"/>
    </owl:NamedIndividual>
    


    <!-- http://purl.bdrc.io/resource/KinFather -->

    <owl:NamedIndividual rdf:about="http://purl.bdrc.io/resource/KinFather">
        <rdf:type rdf:resource="http://purl.bdrc.io/ontology/KinType"/>
        <taxElementOf rdf:resource="http://purl.bdrc.io/resource/KinParent"/>
    </owl:NamedIndividual>
    


    <!-- http://purl.bdrc.io/resource/KinFatherInLaw -->

    <owl:NamedIndividual rdf:about="http://purl.bdrc.io/resource/KinFatherInLaw">
        <rdf:type rdf:resource="http://purl.bdrc.io/ontology/KinType"/>
        <taxElementOf rdf:resource="http://purl.bdrc.io/resource/KinInLaw"/>
    </owl:NamedIndividual>
    


    <!-- http://purl.bdrc.io/resource/KinGrandchild -->

    <owl:NamedIndividual rdf:about="http://purl.bdrc.io/resource/KinGrandchild">
        <rdf:type rdf:resource="http://purl.bdrc.io/ontology/KinType"/>
        <taxSubClass rdf:resource="http://purl.bdrc.io/resource/KinshipTaxonomy"/>
    </owl:NamedIndividual>
    


    <!-- http://purl.bdrc.io/resource/KinGranddaughter -->

    <owl:NamedIndividual rdf:about="http://purl.bdrc.io/resource/KinGranddaughter">
        <rdf:type rdf:resource="http://purl.bdrc.io/ontology/KinType"/>
        <taxElementOf rdf:resource="http://purl.bdrc.io/resource/KinGrandchild"/>
    </owl:NamedIndividual>
    


    <!-- http://purl.bdrc.io/resource/KinGrandfather -->

    <owl:NamedIndividual rdf:about="http://purl.bdrc.io/resource/KinGrandfather">
        <rdf:type rdf:resource="http://purl.bdrc.io/ontology/KinType"/>
        <taxElementOf rdf:resource="http://purl.bdrc.io/resource/KinGrandparent"/>
    </owl:NamedIndividual>
    


    <!-- http://purl.bdrc.io/resource/KinGrandmother -->

    <owl:NamedIndividual rdf:about="http://purl.bdrc.io/resource/KinGrandmother">
        <rdf:type rdf:resource="http://purl.bdrc.io/ontology/KinType"/>
        <taxElementOf rdf:resource="http://purl.bdrc.io/resource/KinGrandparent"/>
    </owl:NamedIndividual>
    


    <!-- http://purl.bdrc.io/resource/KinGrandparent -->

    <owl:NamedIndividual rdf:about="http://purl.bdrc.io/resource/KinGrandparent">
        <rdf:type rdf:resource="http://purl.bdrc.io/ontology/KinType"/>
        <taxSubClass rdf:resource="http://purl.bdrc.io/resource/KinshipTaxonomy"/>
    </owl:NamedIndividual>
    


    <!-- http://purl.bdrc.io/resource/KinGrandson -->

    <owl:NamedIndividual rdf:about="http://purl.bdrc.io/resource/KinGrandson">
        <rdf:type rdf:resource="http://purl.bdrc.io/ontology/KinType"/>
        <taxElementOf rdf:resource="http://purl.bdrc.io/resource/KinGrandchild"/>
    </owl:NamedIndividual>
    


    <!-- http://purl.bdrc.io/resource/KinHusband -->

    <owl:NamedIndividual rdf:about="http://purl.bdrc.io/resource/KinHusband">
        <rdf:type rdf:resource="http://purl.bdrc.io/ontology/KinType"/>
        <taxElementOf rdf:resource="http://purl.bdrc.io/resource/KinSpouse"/>
    </owl:NamedIndividual>
    


    <!-- http://purl.bdrc.io/resource/KinInLaw -->

    <owl:NamedIndividual rdf:about="http://purl.bdrc.io/resource/KinInLaw">
        <rdf:type rdf:resource="http://purl.bdrc.io/ontology/KinType"/>
        <taxSubClass rdf:resource="http://purl.bdrc.io/resource/KinshipTaxonomy"/>
    </owl:NamedIndividual>
    


    <!-- http://purl.bdrc.io/resource/KinMaternalAunt -->

    <owl:NamedIndividual rdf:about="http://purl.bdrc.io/resource/KinMaternalAunt">
        <rdf:type rdf:resource="http://purl.bdrc.io/ontology/KinType"/>
        <taxElementOf rdf:resource="http://purl.bdrc.io/resource/KinAunt"/>
    </owl:NamedIndividual>
    


    <!-- http://purl.bdrc.io/resource/KinMaternalUncle -->

    <owl:NamedIndividual rdf:about="http://purl.bdrc.io/resource/KinMaternalUncle">
        <rdf:type rdf:resource="http://purl.bdrc.io/ontology/KinType"/>
        <taxElementOf rdf:resource="http://purl.bdrc.io/resource/KinUncle"/>
    </owl:NamedIndividual>
    


    <!-- http://purl.bdrc.io/resource/KinMother -->

    <owl:NamedIndividual rdf:about="http://purl.bdrc.io/resource/KinMother">
        <rdf:type rdf:resource="http://purl.bdrc.io/ontology/KinType"/>
        <taxElementOf rdf:resource="http://purl.bdrc.io/resource/KinParent"/>
    </owl:NamedIndividual>
    


    <!-- http://purl.bdrc.io/resource/KinMotherInLaw -->

    <owl:NamedIndividual rdf:about="http://purl.bdrc.io/resource/KinMotherInLaw">
        <rdf:type rdf:resource="http://purl.bdrc.io/ontology/KinType"/>
        <taxElementOf rdf:resource="http://purl.bdrc.io/resource/KinInLaw"/>
    </owl:NamedIndividual>
    


    <!-- http://purl.bdrc.io/resource/KinNephew -->

    <owl:NamedIndividual rdf:about="http://purl.bdrc.io/resource/KinNephew">
        <rdf:type rdf:resource="http://purl.bdrc.io/ontology/KinType"/>
        <taxElementOf rdf:resource="http://purl.bdrc.io/resource/KinNibling"/>
    </owl:NamedIndividual>
    


    <!-- http://purl.bdrc.io/resource/KinNibling -->

    <owl:NamedIndividual rdf:about="http://purl.bdrc.io/resource/KinNibling">
        <rdf:type rdf:resource="http://purl.bdrc.io/ontology/KinType"/>
        <taxSubClass rdf:resource="http://purl.bdrc.io/resource/KinshipTaxonomy"/>
    </owl:NamedIndividual>
    


    <!-- http://purl.bdrc.io/resource/KinNiece -->

    <owl:NamedIndividual rdf:about="http://purl.bdrc.io/resource/KinNiece">
        <rdf:type rdf:resource="http://purl.bdrc.io/ontology/KinType"/>
        <taxElementOf rdf:resource="http://purl.bdrc.io/resource/KinNibling"/>
    </owl:NamedIndividual>
    


    <!-- http://purl.bdrc.io/resource/KinOlderBrother -->

    <owl:NamedIndividual rdf:about="http://purl.bdrc.io/resource/KinOlderBrother">
        <rdf:type rdf:resource="http://purl.bdrc.io/ontology/KinType"/>
        <taxElementOf rdf:resource="http://purl.bdrc.io/resource/KinBrother"/>
    </owl:NamedIndividual>
    


    <!-- http://purl.bdrc.io/resource/KinOlderSister -->

    <owl:NamedIndividual rdf:about="http://purl.bdrc.io/resource/KinOlderSister">
        <rdf:type rdf:resource="http://purl.bdrc.io/ontology/KinType"/>
        <taxElementOf rdf:resource="http://purl.bdrc.io/resource/KinSister"/>
    </owl:NamedIndividual>
    


    <!-- http://purl.bdrc.io/resource/KinParent -->

    <owl:NamedIndividual rdf:about="http://purl.bdrc.io/resource/KinParent">
        <rdf:type rdf:resource="http://purl.bdrc.io/ontology/KinType"/>
        <taxSubClass rdf:resource="http://purl.bdrc.io/resource/KinshipTaxonomy"/>
    </owl:NamedIndividual>
    


    <!-- http://purl.bdrc.io/resource/KinParentSibling -->

    <owl:NamedIndividual rdf:about="http://purl.bdrc.io/resource/KinParentSibling">
        <rdf:type rdf:resource="http://purl.bdrc.io/ontology/KinType"/>
        <taxSubClass rdf:resource="http://purl.bdrc.io/resource/KinshipTaxonomy"/>
    </owl:NamedIndividual>
    


    <!-- http://purl.bdrc.io/resource/KinPaternalAunt -->

    <owl:NamedIndividual rdf:about="http://purl.bdrc.io/resource/KinPaternalAunt">
        <rdf:type rdf:resource="http://purl.bdrc.io/ontology/KinType"/>
        <taxElementOf rdf:resource="http://purl.bdrc.io/resource/KinAunt"/>
    </owl:NamedIndividual>
    


    <!-- http://purl.bdrc.io/resource/KinPaternalUncle -->

    <owl:NamedIndividual rdf:about="http://purl.bdrc.io/resource/KinPaternalUncle">
        <rdf:type rdf:resource="http://purl.bdrc.io/ontology/KinType"/>
        <taxElementOf rdf:resource="http://purl.bdrc.io/resource/KinUncle"/>
    </owl:NamedIndividual>
    


    <!-- http://purl.bdrc.io/resource/KinSibling -->

    <owl:NamedIndividual rdf:about="http://purl.bdrc.io/resource/KinSibling">
        <rdf:type rdf:resource="http://purl.bdrc.io/ontology/KinType"/>
        <taxSubClass rdf:resource="http://purl.bdrc.io/resource/KinshipTaxonomy"/>
    </owl:NamedIndividual>
    


    <!-- http://purl.bdrc.io/resource/KinSister -->

    <owl:NamedIndividual rdf:about="http://purl.bdrc.io/resource/KinSister">
        <rdf:type rdf:resource="http://purl.bdrc.io/ontology/KinType"/>
        <taxSubClass rdf:resource="http://purl.bdrc.io/resource/KinSibling"/>
    </owl:NamedIndividual>
    


    <!-- http://purl.bdrc.io/resource/KinSon -->

    <owl:NamedIndividual rdf:about="http://purl.bdrc.io/resource/KinSon">
        <rdf:type rdf:resource="http://purl.bdrc.io/ontology/KinType"/>
        <taxElementOf rdf:resource="http://purl.bdrc.io/resource/KinChild"/>
    </owl:NamedIndividual>
    


    <!-- http://purl.bdrc.io/resource/KinSonInLaw -->

    <owl:NamedIndividual rdf:about="http://purl.bdrc.io/resource/KinSonInLaw">
        <rdf:type rdf:resource="http://purl.bdrc.io/ontology/KinType"/>
        <taxElementOf rdf:resource="http://purl.bdrc.io/resource/KinInLaw"/>
    </owl:NamedIndividual>
    


    <!-- http://purl.bdrc.io/resource/KinSpouse -->

    <owl:NamedIndividual rdf:about="http://purl.bdrc.io/resource/KinSpouse">
        <rdf:type rdf:resource="http://purl.bdrc.io/ontology/KinType"/>
        <taxSubClass rdf:resource="http://purl.bdrc.io/resource/KinshipTaxonomy"/>
    </owl:NamedIndividual>
    


    <!-- http://purl.bdrc.io/resource/KinUncle -->

    <owl:NamedIndividual rdf:about="http://purl.bdrc.io/resource/KinUncle">
        <rdf:type rdf:resource="http://purl.bdrc.io/ontology/KinType"/>
        <taxSubClass rdf:resource="http://purl.bdrc.io/resource/KinParentSibling"/>
    </owl:NamedIndividual>
    


    <!-- http://purl.bdrc.io/resource/KinUnspecified -->

    <owl:NamedIndividual rdf:about="http://purl.bdrc.io/resource/KinUnspecified">
        <rdf:type rdf:resource="http://purl.bdrc.io/ontology/KinType"/>
        <taxElementOf rdf:resource="http://purl.bdrc.io/resource/KinshipTaxonomy"/>
    </owl:NamedIndividual>
    


    <!-- http://purl.bdrc.io/resource/KinWife -->

    <owl:NamedIndividual rdf:about="http://purl.bdrc.io/resource/KinWife">
        <rdf:type rdf:resource="http://purl.bdrc.io/ontology/KinType"/>
        <taxElementOf rdf:resource="http://purl.bdrc.io/resource/KinSpouse"/>
    </owl:NamedIndividual>
    


    <!-- http://purl.bdrc.io/resource/KinYoungerBrother -->

    <owl:NamedIndividual rdf:about="http://purl.bdrc.io/resource/KinYoungerBrother">
        <rdf:type rdf:resource="http://purl.bdrc.io/ontology/KinType"/>
        <taxElementOf rdf:resource="http://purl.bdrc.io/resource/KinBrother"/>
    </owl:NamedIndividual>
    


    <!-- http://purl.bdrc.io/resource/KinYoungerSister -->

    <owl:NamedIndividual rdf:about="http://purl.bdrc.io/resource/KinYoungerSister">
        <rdf:type rdf:resource="http://purl.bdrc.io/ontology/KinType"/>
        <taxElementOf rdf:resource="http://purl.bdrc.io/resource/KinSister"/>
    </owl:NamedIndividual>
    


    <!-- http://purl.bdrc.io/resource/KinshipTaxonomy -->

    <owl:NamedIndividual rdf:about="http://purl.bdrc.io/resource/KinshipTaxonomy">
        <rdf:type rdf:resource="http://purl.bdrc.io/ontology/Taxonomy"/>
        <taxElementOfRelation rdf:resource="http://purl.bdrc.io/ontology/taxElementOf"/>
        <taxSubclassRelation rdf:resource="http://purl.bdrc.io/ontology/taxSubClass"/>
        <rdfs:comment xml:lang="en">The bdr:KinshipTaxonomy is used to organize the individuals of :Type :KinType.

The relations that are used to organize the :KinType individuals are the :taxElementOf and :taxSubclass properties.</rdfs:comment>
        <rdfs:label xml:lang="en">Kinship Taxonomy</rdfs:label>
    </owl:NamedIndividual>
    


    <!-- http://purl.bdrc.io/resource/LineageDbang -->

    <owl:NamedIndividual rdf:about="http://purl.bdrc.io/resource/LineageDbang">
        <rdf:type rdf:resource="http://purl.bdrc.io/ontology/LineageType"/>
        <rdfs:label xml:lang="en">empowerment</rdfs:label>
    </owl:NamedIndividual>
    


    <!-- http://purl.bdrc.io/resource/LineageDmarKhrid -->

    <owl:NamedIndividual rdf:about="http://purl.bdrc.io/resource/LineageDmarKhrid">
        <rdf:type rdf:resource="http://purl.bdrc.io/ontology/LineageType"/>
        <rdfs:label xml:lang="en">essential instruction</rdfs:label>
    </owl:NamedIndividual>
    


    <!-- http://purl.bdrc.io/resource/LineageGdamsNgag -->

    <owl:NamedIndividual rdf:about="http://purl.bdrc.io/resource/LineageGdamsNgag">
        <rdf:type rdf:resource="http://purl.bdrc.io/ontology/LineageType"/>
        <rdfs:label xml:lang="en">oral instruction</rdfs:label>
    </owl:NamedIndividual>
    


    <!-- http://purl.bdrc.io/resource/LineageKhrid -->

    <owl:NamedIndividual rdf:about="http://purl.bdrc.io/resource/LineageKhrid">
        <rdf:type rdf:resource="http://purl.bdrc.io/ontology/LineageType"/>
        <rdfs:label xml:lang="en">instruction</rdfs:label>
    </owl:NamedIndividual>
    


    <!-- http://purl.bdrc.io/resource/LineageLung -->

    <owl:NamedIndividual rdf:about="http://purl.bdrc.io/resource/LineageLung">
        <rdf:type rdf:resource="http://purl.bdrc.io/ontology/LineageType"/>
        <rdfs:label xml:lang="en">reading transmission</rdfs:label>
    </owl:NamedIndividual>
    


    <!-- http://purl.bdrc.io/resource/LineageManNgag -->

    <owl:NamedIndividual rdf:about="http://purl.bdrc.io/resource/LineageManNgag">
        <rdf:type rdf:resource="http://purl.bdrc.io/ontology/LineageType"/>
        <rdfs:label xml:lang="en">quintessential instruction</rdfs:label>
    </owl:NamedIndividual>
    


    <!-- http://purl.bdrc.io/resource/LineageNotSpecified -->

    <owl:NamedIndividual rdf:about="http://purl.bdrc.io/resource/LineageNotSpecified">
        <rdf:type rdf:resource="http://purl.bdrc.io/ontology/LineageType"/>
        <rdfs:label xml:lang="en">not specified</rdfs:label>
    </owl:NamedIndividual>
    


    <!-- http://purl.bdrc.io/resource/LineageNyeBrgyud -->

    <owl:NamedIndividual rdf:about="http://purl.bdrc.io/resource/LineageNyeBrgyud">
        <rdf:type rdf:resource="http://purl.bdrc.io/ontology/LineageType"/>
        <rdfs:label xml:lang="en">direct transmission</rdfs:label>
    </owl:NamedIndividual>
    


    <!-- http://purl.bdrc.io/resource/LineageRingBrgyud -->

    <owl:NamedIndividual rdf:about="http://purl.bdrc.io/resource/LineageRingBrgyud">
        <rdf:type rdf:resource="http://purl.bdrc.io/ontology/LineageType"/>
        <rdfs:label xml:lang="en">long lineage transmission</rdfs:label>
    </owl:NamedIndividual>
    


    <!-- http://purl.bdrc.io/resource/LineageRjesGnang -->

    <owl:NamedIndividual rdf:about="http://purl.bdrc.io/resource/LineageRjesGnang">
        <rdf:type rdf:resource="http://purl.bdrc.io/ontology/LineageType"/>
        <rdfs:label xml:lang="en">short empowerment</rdfs:label>
    </owl:NamedIndividual>
    


    <!-- http://purl.bdrc.io/resource/LineageSdomBrgyud -->

    <owl:NamedIndividual rdf:about="http://purl.bdrc.io/resource/LineageSdomBrgyud">
        <rdf:type rdf:resource="http://purl.bdrc.io/ontology/LineageType"/>
        <rdfs:label xml:lang="en">lineage of vows</rdfs:label>
    </owl:NamedIndividual>
    


    <!-- http://purl.bdrc.io/resource/LineageSnyanBrgyud -->

    <owl:NamedIndividual rdf:about="http://purl.bdrc.io/resource/LineageSnyanBrgyud">
        <rdf:type rdf:resource="http://purl.bdrc.io/ontology/LineageType"/>
        <rdfs:label xml:lang="en">oral lineage</rdfs:label>
    </owl:NamedIndividual>
    


    <!-- http://purl.bdrc.io/resource/OutlineTypeCompositeVolume -->

    <owl:NamedIndividual rdf:about="http://purl.bdrc.io/resource/OutlineTypeCompositeVolume">
        <rdf:type rdf:resource="http://purl.bdrc.io/ontology/OutlineType"/>
    </owl:NamedIndividual>
    


    <!-- http://purl.bdrc.io/resource/OutlineTypeGsungBum -->

    <owl:NamedIndividual rdf:about="http://purl.bdrc.io/resource/OutlineTypeGsungBum">
        <rdf:type rdf:resource="http://purl.bdrc.io/ontology/OutlineType"/>
    </owl:NamedIndividual>
    


    <!-- http://purl.bdrc.io/resource/OutlineTypeGterChos -->

    <owl:NamedIndividual rdf:about="http://purl.bdrc.io/resource/OutlineTypeGterChos">
        <rdf:type rdf:resource="http://purl.bdrc.io/ontology/OutlineType"/>
    </owl:NamedIndividual>
    


    <!-- http://purl.bdrc.io/resource/OutlineTypeMultiVolumeCollection -->

    <owl:NamedIndividual rdf:about="http://purl.bdrc.io/resource/OutlineTypeMultiVolumeCollection">
        <rdf:type rdf:resource="http://purl.bdrc.io/ontology/OutlineType"/>
    </owl:NamedIndividual>
    


    <!-- http://purl.bdrc.io/resource/OutlineTypeNotAssigned -->

    <owl:NamedIndividual rdf:about="http://purl.bdrc.io/resource/OutlineTypeNotAssigned">
        <rdf:type rdf:resource="http://purl.bdrc.io/ontology/OutlineType"/>
    </owl:NamedIndividual>
    


    <!-- http://purl.bdrc.io/resource/OutlineTypePartialCollectedWorks -->

    <owl:NamedIndividual rdf:about="http://purl.bdrc.io/resource/OutlineTypePartialCollectedWorks">
        <rdf:type rdf:resource="http://purl.bdrc.io/ontology/OutlineType"/>
    </owl:NamedIndividual>
    


    <!-- http://purl.bdrc.io/resource/OutlineTypeSaBcad -->

    <owl:NamedIndividual rdf:about="http://purl.bdrc.io/resource/OutlineTypeSaBcad">
        <rdf:type rdf:resource="http://purl.bdrc.io/ontology/OutlineType"/>
    </owl:NamedIndividual>
    


    <!-- http://purl.bdrc.io/resource/OutlineTypeSubjectCollection -->

    <owl:NamedIndividual rdf:about="http://purl.bdrc.io/resource/OutlineTypeSubjectCollection">
        <rdf:type rdf:resource="http://purl.bdrc.io/ontology/OutlineType"/>
    </owl:NamedIndividual>
    


    <!-- http://purl.bdrc.io/resource/PaginationAbsolute -->

    <owl:NamedIndividual rdf:about="http://purl.bdrc.io/resource/PaginationAbsolute">
        <rdf:type rdf:resource="http://purl.bdrc.io/ontology/PaginationType"/>
        <rdfs:label xml:lang="en">absolute pagination</rdfs:label>
    </owl:NamedIndividual>
    


    <!-- http://purl.bdrc.io/resource/PaginationRelative -->

    <owl:NamedIndividual rdf:about="http://purl.bdrc.io/resource/PaginationRelative">
        <rdf:type rdf:resource="http://purl.bdrc.io/ontology/PaginationType"/>
        <rdfs:label xml:lang="en">relative pagination</rdfs:label>
    </owl:NamedIndividual>
    


    <!-- http://purl.bdrc.io/resource/PersonBodhisattvaVowName -->

    <owl:NamedIndividual rdf:about="http://purl.bdrc.io/resource/PersonBodhisattvaVowName">
        <rdf:type rdf:resource="http://purl.bdrc.io/ontology/PersonNameType"/>
    </owl:NamedIndividual>
    


    <!-- http://purl.bdrc.io/resource/PersonChineseName -->

    <owl:NamedIndividual rdf:about="http://purl.bdrc.io/resource/PersonChineseName">
        <rdf:type rdf:resource="http://purl.bdrc.io/ontology/PersonNameType"/>
    </owl:NamedIndividual>
    


    <!-- http://purl.bdrc.io/resource/PersonCommonName -->

    <owl:NamedIndividual rdf:about="http://purl.bdrc.io/resource/PersonCommonName">
        <rdf:type rdf:resource="http://purl.bdrc.io/ontology/PersonNameType"/>
    </owl:NamedIndividual>
    


    <!-- http://purl.bdrc.io/resource/PersonCorporateName -->

    <owl:NamedIndividual rdf:about="http://purl.bdrc.io/resource/PersonCorporateName">
        <rdf:type rdf:resource="http://purl.bdrc.io/ontology/PersonNameType"/>
    </owl:NamedIndividual>
    


    <!-- http://purl.bdrc.io/resource/PersonEventAffiliation -->

    <owl:NamedIndividual rdf:about="http://purl.bdrc.io/resource/PersonEventAffiliation">
        <rdf:type rdf:resource="http://purl.bdrc.io/ontology/PersonEventType"/>
        <rdfs:label xml:lang="en">Affiliation</rdfs:label>
    </owl:NamedIndividual>
    


    <!-- http://purl.bdrc.io/resource/PersonEventAssumesOffice -->

    <owl:NamedIndividual rdf:about="http://purl.bdrc.io/resource/PersonEventAssumesOffice">
        <rdf:type rdf:resource="http://purl.bdrc.io/ontology/PersonEventType"/>
        <rdfs:label xml:lang="en">Assumes Office</rdfs:label>
    </owl:NamedIndividual>
    


    <!-- http://purl.bdrc.io/resource/PersonEventAssumesSeat -->

    <owl:NamedIndividual rdf:about="http://purl.bdrc.io/resource/PersonEventAssumesSeat">
        <rdf:type rdf:resource="http://purl.bdrc.io/ontology/PersonEventType"/>
        <rdfs:label xml:lang="en">Assumes Seat</rdfs:label>
    </owl:NamedIndividual>
    


    <!-- http://purl.bdrc.io/resource/PersonEventBirth -->

    <owl:NamedIndividual rdf:about="http://purl.bdrc.io/resource/PersonEventBirth">
        <rdf:type rdf:resource="http://purl.bdrc.io/ontology/PersonEventType"/>
        <rdfs:label xml:lang="en">Birth</rdfs:label>
    </owl:NamedIndividual>
    


    <!-- http://purl.bdrc.io/resource/PersonEventDeath -->

    <owl:NamedIndividual rdf:about="http://purl.bdrc.io/resource/PersonEventDeath">
        <rdf:type rdf:resource="http://purl.bdrc.io/ontology/PersonEventType"/>
        <rdfs:label xml:lang="en">Death</rdfs:label>
    </owl:NamedIndividual>
    


    <!-- http://purl.bdrc.io/resource/PersonEventDivorce -->

    <owl:NamedIndividual rdf:about="http://purl.bdrc.io/resource/PersonEventDivorce">
        <rdf:type rdf:resource="http://purl.bdrc.io/ontology/PersonEventType"/>
        <rdfs:label xml:lang="en">Dviorce</rdfs:label>
    </owl:NamedIndividual>
    


    <!-- http://purl.bdrc.io/resource/PersonEventFinalOrdination -->

    <owl:NamedIndividual rdf:about="http://purl.bdrc.io/resource/PersonEventFinalOrdination">
        <rdf:type rdf:resource="http://purl.bdrc.io/ontology/PersonEventType"/>
        <rdfs:label xml:lang="en">Final Ordination</rdfs:label>
    </owl:NamedIndividual>
    


    <!-- http://purl.bdrc.io/resource/PersonEventGterMaDiscovery -->

    <owl:NamedIndividual rdf:about="http://purl.bdrc.io/resource/PersonEventGterMaDiscovery">
        <rdf:type rdf:resource="http://purl.bdrc.io/ontology/PersonEventType"/>
        <rdfs:label xml:lang="en">Discovers Terma</rdfs:label>
    </owl:NamedIndividual>
    


    <!-- http://purl.bdrc.io/resource/PersonEventInResidence -->

    <owl:NamedIndividual rdf:about="http://purl.bdrc.io/resource/PersonEventInResidence">
        <rdf:type rdf:resource="http://purl.bdrc.io/ontology/PersonEventType"/>
        <rdfs:label xml:lang="en">In Residence</rdfs:label>
    </owl:NamedIndividual>
    


    <!-- http://purl.bdrc.io/resource/PersonEventLeavesOffice -->

    <owl:NamedIndividual rdf:about="http://purl.bdrc.io/resource/PersonEventLeavesOffice">
        <rdf:type rdf:resource="http://purl.bdrc.io/ontology/PersonEventType"/>
        <rdfs:label xml:lang="en">Leaves Office</rdfs:label>
    </owl:NamedIndividual>
    


    <!-- http://purl.bdrc.io/resource/PersonEventLeavesSeat -->

    <owl:NamedIndividual rdf:about="http://purl.bdrc.io/resource/PersonEventLeavesSeat">
        <rdf:type rdf:resource="http://purl.bdrc.io/ontology/PersonEventType"/>
        <rdfs:label xml:lang="en">Leaves Seat</rdfs:label>
    </owl:NamedIndividual>
    


    <!-- http://purl.bdrc.io/resource/PersonEventMarriage -->

    <owl:NamedIndividual rdf:about="http://purl.bdrc.io/resource/PersonEventMarriage">
        <rdf:type rdf:resource="http://purl.bdrc.io/ontology/PersonEventType"/>
        <rdfs:label xml:lang="en">Marriage</rdfs:label>
    </owl:NamedIndividual>
    


    <!-- http://purl.bdrc.io/resource/PersonEventMonasteryFoundation -->

    <owl:NamedIndividual rdf:about="http://purl.bdrc.io/resource/PersonEventMonasteryFoundation">
        <rdf:type rdf:resource="http://purl.bdrc.io/ontology/PersonEventType"/>
        <rdfs:label xml:lang="en">Founds Monastery</rdfs:label>
    </owl:NamedIndividual>
    


    <!-- http://purl.bdrc.io/resource/PersonEventNotSpecified -->

    <owl:NamedIndividual rdf:about="http://purl.bdrc.io/resource/PersonEventNotSpecified">
        <rdf:type rdf:resource="http://purl.bdrc.io/ontology/PersonEventType"/>
        <rdfs:label xml:lang="en">Not Specified</rdfs:label>
    </owl:NamedIndividual>
    


    <!-- http://purl.bdrc.io/resource/PersonEventOccupiesSeat -->

    <owl:NamedIndividual rdf:about="http://purl.bdrc.io/resource/PersonEventOccupiesSeat">
        <rdf:type rdf:resource="http://purl.bdrc.io/ontology/PersonEventType"/>
        <rdfs:comment xml:lang="en">Migration hint: Rather than a separate :personHasSeat property, the &lt;p:seat/&gt; is modeled as a PersonEventOccupiesSeat with the place and circa as for any other PersonEvent</rdfs:comment>
        <rdfs:label xml:lang="en">Occupies Seat</rdfs:label>
    </owl:NamedIndividual>
    


    <!-- http://purl.bdrc.io/resource/PersonEventRabByungOrdination -->

    <owl:NamedIndividual rdf:about="http://purl.bdrc.io/resource/PersonEventRabByungOrdination">
        <rdf:type rdf:resource="http://purl.bdrc.io/ontology/PersonEventType"/>
        <rdfs:label xml:lang="en">Rabjung Ordination</rdfs:label>
    </owl:NamedIndividual>
    


    <!-- http://purl.bdrc.io/resource/PersonFamilyName -->

    <owl:NamedIndividual rdf:about="http://purl.bdrc.io/resource/PersonFamilyName">
        <rdf:type rdf:resource="http://purl.bdrc.io/ontology/PersonNameType"/>
    </owl:NamedIndividual>
    


    <!-- http://purl.bdrc.io/resource/PersonFinalOrdinationName -->

    <owl:NamedIndividual rdf:about="http://purl.bdrc.io/resource/PersonFinalOrdinationName">
        <rdf:type rdf:resource="http://purl.bdrc.io/ontology/PersonNameType"/>
    </owl:NamedIndividual>
    


    <!-- http://purl.bdrc.io/resource/PersonFirstOrdinationName -->

    <owl:NamedIndividual rdf:about="http://purl.bdrc.io/resource/PersonFirstOrdinationName">
        <rdf:type rdf:resource="http://purl.bdrc.io/ontology/PersonNameType"/>
    </owl:NamedIndividual>
    


    <!-- http://purl.bdrc.io/resource/PersonGterStonTitle -->

    <owl:NamedIndividual rdf:about="http://purl.bdrc.io/resource/PersonGterStonTitle">
        <rdf:type rdf:resource="http://purl.bdrc.io/ontology/PersonNameType"/>
    </owl:NamedIndividual>
    


    <!-- http://purl.bdrc.io/resource/PersonOfficeTitle -->

    <owl:NamedIndividual rdf:about="http://purl.bdrc.io/resource/PersonOfficeTitle">
        <rdf:type rdf:resource="http://purl.bdrc.io/ontology/PersonNameType"/>
    </owl:NamedIndividual>
    


    <!-- http://purl.bdrc.io/resource/PersonOtherName -->

    <owl:NamedIndividual rdf:about="http://purl.bdrc.io/resource/PersonOtherName">
        <rdf:type rdf:resource="http://purl.bdrc.io/ontology/PersonNameType"/>
    </owl:NamedIndividual>
    


    <!-- http://purl.bdrc.io/resource/PersonPenName -->

    <owl:NamedIndividual rdf:about="http://purl.bdrc.io/resource/PersonPenName">
        <rdf:type rdf:resource="http://purl.bdrc.io/ontology/PersonNameType"/>
    </owl:NamedIndividual>
    


    <!-- http://purl.bdrc.io/resource/PersonPersonTitle -->

    <owl:NamedIndividual rdf:about="http://purl.bdrc.io/resource/PersonPersonTitle">
        <rdf:type rdf:resource="http://purl.bdrc.io/ontology/PersonNameType"/>
    </owl:NamedIndividual>
    


    <!-- http://purl.bdrc.io/resource/PersonPersonalName -->

    <owl:NamedIndividual rdf:about="http://purl.bdrc.io/resource/PersonPersonalName">
        <rdf:type rdf:resource="http://purl.bdrc.io/ontology/PersonNameType"/>
    </owl:NamedIndividual>
    


    <!-- http://purl.bdrc.io/resource/PersonPrimaryName -->

    <owl:NamedIndividual rdf:about="http://purl.bdrc.io/resource/PersonPrimaryName">
        <rdf:type rdf:resource="http://purl.bdrc.io/ontology/PersonNameType"/>
    </owl:NamedIndividual>
    


    <!-- http://purl.bdrc.io/resource/PersonPrimaryTitle -->

    <owl:NamedIndividual rdf:about="http://purl.bdrc.io/resource/PersonPrimaryTitle">
        <rdf:type rdf:resource="http://purl.bdrc.io/ontology/PersonNameType"/>
    </owl:NamedIndividual>
    


    <!-- http://purl.bdrc.io/resource/PersonSecretInitiatoryName -->

    <owl:NamedIndividual rdf:about="http://purl.bdrc.io/resource/PersonSecretInitiatoryName">
        <rdf:type rdf:resource="http://purl.bdrc.io/ontology/PersonNameType"/>
    </owl:NamedIndividual>
    


    <!-- http://purl.bdrc.io/resource/PersonTulkuTitle -->

    <owl:NamedIndividual rdf:about="http://purl.bdrc.io/resource/PersonTulkuTitle">
        <rdf:type rdf:resource="http://purl.bdrc.io/ontology/PersonNameType"/>
    </owl:NamedIndividual>
    


    <!-- http://purl.bdrc.io/resource/PlaceAbandoned -->

    <owl:NamedIndividual rdf:about="http://purl.bdrc.io/resource/PlaceAbandoned">
        <rdf:type rdf:resource="http://purl.bdrc.io/ontology/PlaceEventType"/>
        <rdfs:label xml:lang="en">abandoned</rdfs:label>
    </owl:NamedIndividual>
    


    <!-- http://purl.bdrc.io/resource/PlaceConverted -->

    <owl:NamedIndividual rdf:about="http://purl.bdrc.io/resource/PlaceConverted">
        <rdf:type rdf:resource="http://purl.bdrc.io/ontology/PlaceEventType"/>
        <rdfs:label xml:lang="en">converted</rdfs:label>
    </owl:NamedIndividual>
    


    <!-- http://purl.bdrc.io/resource/PlaceDestroyed -->

    <owl:NamedIndividual rdf:about="http://purl.bdrc.io/resource/PlaceDestroyed">
        <rdf:type rdf:resource="http://purl.bdrc.io/ontology/PlaceEventType"/>
        <rdfs:label xml:lang="en">destroyed</rdfs:label>
    </owl:NamedIndividual>
    


    <!-- http://purl.bdrc.io/resource/PlaceEventTypeNotSpecified -->

    <owl:NamedIndividual rdf:about="http://purl.bdrc.io/resource/PlaceEventTypeNotSpecified">
        <rdf:type rdf:resource="http://purl.bdrc.io/ontology/PlaceEventType"/>
        <rdfs:label xml:lang="en">not specified</rdfs:label>
    </owl:NamedIndividual>
    


    <!-- http://purl.bdrc.io/resource/PlaceFounded -->

    <owl:NamedIndividual rdf:about="http://purl.bdrc.io/resource/PlaceFounded">
        <rdf:type rdf:resource="http://purl.bdrc.io/ontology/PlaceEventType"/>
        <rdfs:label xml:lang="en">founded</rdfs:label>
    </owl:NamedIndividual>
    


    <!-- http://purl.bdrc.io/resource/PlaceRebuilt -->

    <owl:NamedIndividual rdf:about="http://purl.bdrc.io/resource/PlaceRebuilt">
        <rdf:type rdf:resource="http://purl.bdrc.io/ontology/PlaceEventType"/>
        <rdfs:label xml:lang="en">rebuilt</rdfs:label>
    </owl:NamedIndividual>
    


    <!-- http://purl.bdrc.io/resource/PlaceTypeBangSo -->

    <owl:NamedIndividual rdf:about="http://purl.bdrc.io/resource/PlaceTypeBangSo">
        <rdf:type rdf:resource="http://purl.bdrc.io/ontology/PlaceType"/>
    </owl:NamedIndividual>
    


    <!-- http://purl.bdrc.io/resource/PlaceTypeBeHu -->

    <owl:NamedIndividual rdf:about="http://purl.bdrc.io/resource/PlaceTypeBeHu">
        <rdf:type rdf:resource="http://purl.bdrc.io/ontology/PlaceType"/>
    </owl:NamedIndividual>
    


    <!-- http://purl.bdrc.io/resource/PlaceTypeBlaBrang -->

    <owl:NamedIndividual rdf:about="http://purl.bdrc.io/resource/PlaceTypeBlaBrang">
        <rdf:type rdf:resource="http://purl.bdrc.io/ontology/PlaceType"/>
    </owl:NamedIndividual>
    


    <!-- http://purl.bdrc.io/resource/PlaceTypeBrogSde -->

    <owl:NamedIndividual rdf:about="http://purl.bdrc.io/resource/PlaceTypeBrogSde">
        <rdf:type rdf:resource="http://purl.bdrc.io/ontology/PlaceType"/>
    </owl:NamedIndividual>
    


    <!-- http://purl.bdrc.io/resource/PlaceTypeBrtenPaGnasKhang -->

    <owl:NamedIndividual rdf:about="http://purl.bdrc.io/resource/PlaceTypeBrtenPaGnasKhang">
        <rdf:type rdf:resource="http://purl.bdrc.io/ontology/PlaceType"/>
        <rdfs:comment xml:lang="en">Sites of interest such as monasteries, temples and so on</rdfs:comment>
        <rdfs:label xml:lang="en">Sites</rdfs:label>
        <rdfs:label xml:lang="bo-x-ewts">brten pa gnas khang</rdfs:label>
        <rdfs:label xml:lang="zh">场所</rdfs:label>
    </owl:NamedIndividual>
    


    <!-- http://purl.bdrc.io/resource/PlaceTypeBshadGrwa -->

    <owl:NamedIndividual rdf:about="http://purl.bdrc.io/resource/PlaceTypeBshadGrwa">
        <rdf:type rdf:resource="http://purl.bdrc.io/ontology/PlaceType"/>
    </owl:NamedIndividual>
    


    <!-- http://purl.bdrc.io/resource/PlaceTypeBtsunDgon -->

    <owl:NamedIndividual rdf:about="http://purl.bdrc.io/resource/PlaceTypeBtsunDgon">
        <rdf:type rdf:resource="http://purl.bdrc.io/ontology/PlaceType"/>
    </owl:NamedIndividual>
    


    <!-- http://purl.bdrc.io/resource/PlaceTypeCholKha -->

    <owl:NamedIndividual rdf:about="http://purl.bdrc.io/resource/PlaceTypeCholKha">
        <rdf:type rdf:resource="http://purl.bdrc.io/ontology/PlaceType"/>
    </owl:NamedIndividual>
    


    <!-- http://purl.bdrc.io/resource/PlaceTypeChuBo -->

    <owl:NamedIndividual rdf:about="http://purl.bdrc.io/resource/PlaceTypeChuBo">
        <rdf:type rdf:resource="http://purl.bdrc.io/ontology/PlaceType"/>
    </owl:NamedIndividual>
    


    <!-- http://purl.bdrc.io/resource/PlaceTypeChuMig -->

    <owl:NamedIndividual rdf:about="http://purl.bdrc.io/resource/PlaceTypeChuMig">
        <rdf:type rdf:resource="http://purl.bdrc.io/ontology/PlaceType"/>
    </owl:NamedIndividual>
    


    <!-- http://purl.bdrc.io/resource/PlaceTypeChuRgyud -->

    <owl:NamedIndividual rdf:about="http://purl.bdrc.io/resource/PlaceTypeChuRgyud">
        <rdf:type rdf:resource="http://purl.bdrc.io/ontology/PlaceType"/>
    </owl:NamedIndividual>
    


    <!-- http://purl.bdrc.io/resource/PlaceTypeChus -->

    <owl:NamedIndividual rdf:about="http://purl.bdrc.io/resource/PlaceTypeChus">
        <rdf:type rdf:resource="http://purl.bdrc.io/ontology/PlaceType"/>
    </owl:NamedIndividual>
    


    <!-- http://purl.bdrc.io/resource/PlaceTypeDengRabsSaGnas -->

    <owl:NamedIndividual rdf:about="http://purl.bdrc.io/resource/PlaceTypeDengRabsSaGnas">
        <rdf:type rdf:resource="http://purl.bdrc.io/ontology/PlaceType"/>
        <rdfs:comment xml:lang="en">Modern or contemporary places defined in terms of current political control such as Chinese counties, provinces and so on</rdfs:comment>
        <rdfs:label xml:lang="en">Contemporary Places</rdfs:label>
        <rdfs:label xml:lang="bo-x-ewts">deng rabs sa gnas</rdfs:label>
    </owl:NamedIndividual>
    


    <!-- http://purl.bdrc.io/resource/PlaceTypeDgonPa -->

    <owl:NamedIndividual rdf:about="http://purl.bdrc.io/resource/PlaceTypeDgonPa">
        <rdf:type rdf:resource="http://purl.bdrc.io/ontology/PlaceType"/>
    </owl:NamedIndividual>
    


    <!-- http://purl.bdrc.io/resource/PlaceTypeDpeMdzodKhang -->

    <owl:NamedIndividual rdf:about="http://purl.bdrc.io/resource/PlaceTypeDpeMdzodKhang">
        <rdf:type rdf:resource="http://purl.bdrc.io/ontology/PlaceType"/>
    </owl:NamedIndividual>
    


    <!-- http://purl.bdrc.io/resource/PlaceTypeDurKhrod -->

    <owl:NamedIndividual rdf:about="http://purl.bdrc.io/resource/PlaceTypeDurKhrod">
        <rdf:type rdf:resource="http://purl.bdrc.io/ontology/PlaceType"/>
    </owl:NamedIndividual>
    


    <!-- http://purl.bdrc.io/resource/PlaceTypeGling -->

    <owl:NamedIndividual rdf:about="http://purl.bdrc.io/resource/PlaceTypeGling">
        <rdf:type rdf:resource="http://purl.bdrc.io/ontology/PlaceType"/>
    </owl:NamedIndividual>
    


    <!-- http://purl.bdrc.io/resource/PlaceTypeGlingKha -->

    <owl:NamedIndividual rdf:about="http://purl.bdrc.io/resource/PlaceTypeGlingKha">
        <rdf:type rdf:resource="http://purl.bdrc.io/ontology/PlaceType"/>
    </owl:NamedIndividual>
    


    <!-- http://purl.bdrc.io/resource/PlaceTypeGnasChen -->

    <owl:NamedIndividual rdf:about="http://purl.bdrc.io/resource/PlaceTypeGnasChen">
        <rdf:type rdf:resource="http://purl.bdrc.io/ontology/PlaceType"/>
    </owl:NamedIndividual>
    


    <!-- http://purl.bdrc.io/resource/PlaceTypeGrongKhyer -->

    <owl:NamedIndividual rdf:about="http://purl.bdrc.io/resource/PlaceTypeGrongKhyer">
        <rdf:type rdf:resource="http://purl.bdrc.io/ontology/PlaceType"/>
    </owl:NamedIndividual>
    


    <!-- http://purl.bdrc.io/resource/PlaceTypeGrongRdal -->

    <owl:NamedIndividual rdf:about="http://purl.bdrc.io/resource/PlaceTypeGrongRdal">
        <rdf:type rdf:resource="http://purl.bdrc.io/ontology/PlaceType"/>
    </owl:NamedIndividual>
    


    <!-- http://purl.bdrc.io/resource/PlaceTypeGrongSde -->

    <owl:NamedIndividual rdf:about="http://purl.bdrc.io/resource/PlaceTypeGrongSde">
        <rdf:type rdf:resource="http://purl.bdrc.io/ontology/PlaceType"/>
    </owl:NamedIndividual>
    


    <!-- http://purl.bdrc.io/resource/PlaceTypeGrongTsho -->

    <owl:NamedIndividual rdf:about="http://purl.bdrc.io/resource/PlaceTypeGrongTsho">
        <rdf:type rdf:resource="http://purl.bdrc.io/ontology/PlaceType"/>
    </owl:NamedIndividual>
    


    <!-- http://purl.bdrc.io/resource/PlaceTypeGruKha -->

    <owl:NamedIndividual rdf:about="http://purl.bdrc.io/resource/PlaceTypeGruKha">
        <rdf:type rdf:resource="http://purl.bdrc.io/ontology/PlaceType"/>
    </owl:NamedIndividual>
    


    <!-- http://purl.bdrc.io/resource/PlaceTypeGrwaTshang -->

    <owl:NamedIndividual rdf:about="http://purl.bdrc.io/resource/PlaceTypeGrwaTshang">
        <rdf:type rdf:resource="http://purl.bdrc.io/ontology/PlaceType"/>
    </owl:NamedIndividual>
    


    <!-- http://purl.bdrc.io/resource/PlaceTypeGterGnas -->

    <owl:NamedIndividual rdf:about="http://purl.bdrc.io/resource/PlaceTypeGterGnas">
        <rdf:type rdf:resource="http://purl.bdrc.io/ontology/PlaceType"/>
    </owl:NamedIndividual>
    


    <!-- http://purl.bdrc.io/resource/PlaceTypeGtsugLagKhang -->

    <owl:NamedIndividual rdf:about="http://purl.bdrc.io/resource/PlaceTypeGtsugLagKhang">
        <rdf:type rdf:resource="http://purl.bdrc.io/ontology/PlaceType"/>
    </owl:NamedIndividual>
    


    <!-- http://purl.bdrc.io/resource/PlaceTypeGzhisKa -->

    <owl:NamedIndividual rdf:about="http://purl.bdrc.io/resource/PlaceTypeGzhisKa">
        <rdf:type rdf:resource="http://purl.bdrc.io/ontology/PlaceType"/>
    </owl:NamedIndividual>
    


    <!-- http://purl.bdrc.io/resource/PlaceTypeGzimsKhang -->

    <owl:NamedIndividual rdf:about="http://purl.bdrc.io/resource/PlaceTypeGzimsKhang">
        <rdf:type rdf:resource="http://purl.bdrc.io/ontology/PlaceType"/>
    </owl:NamedIndividual>
    


    <!-- http://purl.bdrc.io/resource/PlaceTypeGzimsShag -->

    <owl:NamedIndividual rdf:about="http://purl.bdrc.io/resource/PlaceTypeGzimsShag">
        <rdf:type rdf:resource="http://purl.bdrc.io/ontology/PlaceType"/>
    </owl:NamedIndividual>
    


    <!-- http://purl.bdrc.io/resource/PlaceTypeKhamsTshan -->

    <owl:NamedIndividual rdf:about="http://purl.bdrc.io/resource/PlaceTypeKhamsTshan">
        <rdf:type rdf:resource="http://purl.bdrc.io/ontology/PlaceType"/>
    </owl:NamedIndividual>
    


    <!-- http://purl.bdrc.io/resource/PlaceTypeKhriSde -->

    <owl:NamedIndividual rdf:about="http://purl.bdrc.io/resource/PlaceTypeKhriSde">
        <rdf:type rdf:resource="http://purl.bdrc.io/ontology/PlaceType"/>
    </owl:NamedIndividual>
    


    <!-- http://purl.bdrc.io/resource/PlaceTypeKhriSkor -->

    <owl:NamedIndividual rdf:about="http://purl.bdrc.io/resource/PlaceTypeKhriSkor">
        <rdf:type rdf:resource="http://purl.bdrc.io/ontology/PlaceType"/>
    </owl:NamedIndividual>
    


    <!-- http://purl.bdrc.io/resource/PlaceTypeKhul -->

    <owl:NamedIndividual rdf:about="http://purl.bdrc.io/resource/PlaceTypeKhul">
        <rdf:type rdf:resource="http://purl.bdrc.io/ontology/PlaceType"/>
    </owl:NamedIndividual>
    


    <!-- http://purl.bdrc.io/resource/PlaceTypeKhyimTshang -->

    <owl:NamedIndividual rdf:about="http://purl.bdrc.io/resource/PlaceTypeKhyimTshang">
        <rdf:type rdf:resource="http://purl.bdrc.io/ontology/PlaceType"/>
    </owl:NamedIndividual>
    


    <!-- http://purl.bdrc.io/resource/PlaceTypeLaKha -->

    <owl:NamedIndividual rdf:about="http://purl.bdrc.io/resource/PlaceTypeLaKha">
        <rdf:type rdf:resource="http://purl.bdrc.io/ontology/PlaceType"/>
    </owl:NamedIndividual>
    


    <!-- http://purl.bdrc.io/resource/PlaceTypeLhaKhang -->

    <owl:NamedIndividual rdf:about="http://purl.bdrc.io/resource/PlaceTypeLhaKhang">
        <rdf:type rdf:resource="http://purl.bdrc.io/ontology/PlaceType"/>
    </owl:NamedIndividual>
    


    <!-- http://purl.bdrc.io/resource/PlaceTypeMaNiRdoPhung -->

    <owl:NamedIndividual rdf:about="http://purl.bdrc.io/resource/PlaceTypeMaNiRdoPhung">
        <rdf:type rdf:resource="http://purl.bdrc.io/ontology/PlaceType"/>
    </owl:NamedIndividual>
    


    <!-- http://purl.bdrc.io/resource/PlaceTypeMchodRten -->

    <owl:NamedIndividual rdf:about="http://purl.bdrc.io/resource/PlaceTypeMchodRten">
        <rdf:type rdf:resource="http://purl.bdrc.io/ontology/PlaceType"/>
    </owl:NamedIndividual>
    


    <!-- http://purl.bdrc.io/resource/PlaceTypeMda -->

    <owl:NamedIndividual rdf:about="http://purl.bdrc.io/resource/PlaceTypeMda">
        <rdf:type rdf:resource="http://purl.bdrc.io/ontology/PlaceType"/>
    </owl:NamedIndividual>
    


    <!-- http://purl.bdrc.io/resource/PlaceTypeMkharRnying -->

    <owl:NamedIndividual rdf:about="http://purl.bdrc.io/resource/PlaceTypeMkharRnying">
        <rdf:type rdf:resource="http://purl.bdrc.io/ontology/PlaceType"/>
    </owl:NamedIndividual>
    


    <!-- http://purl.bdrc.io/resource/PlaceTypeMtsho -->

    <owl:NamedIndividual rdf:about="http://purl.bdrc.io/resource/PlaceTypeMtsho">
        <rdf:type rdf:resource="http://purl.bdrc.io/ontology/PlaceType"/>
    </owl:NamedIndividual>
    


    <!-- http://purl.bdrc.io/resource/PlaceTypeNagsTshal -->

    <owl:NamedIndividual rdf:about="http://purl.bdrc.io/resource/PlaceTypeNagsTshal">
        <rdf:type rdf:resource="http://purl.bdrc.io/ontology/PlaceType"/>
    </owl:NamedIndividual>
    


    <!-- http://purl.bdrc.io/resource/PlaceTypeNotSpecified -->

    <owl:NamedIndividual rdf:about="http://purl.bdrc.io/resource/PlaceTypeNotSpecified">
        <rdf:type rdf:resource="http://purl.bdrc.io/ontology/PlaceType"/>
        <rdfs:comment xml:lang="en">Places of unspecified type</rdfs:comment>
        <rdfs:label xml:lang="en">Not Specified</rdfs:label>
    </owl:NamedIndividual>
    


    <!-- http://purl.bdrc.io/resource/PlaceTypeParKhang -->

    <owl:NamedIndividual rdf:about="http://purl.bdrc.io/resource/PlaceTypeParKhang">
        <rdf:type rdf:resource="http://purl.bdrc.io/ontology/PlaceType"/>
    </owl:NamedIndividual>
    


    <!-- http://purl.bdrc.io/resource/PlaceTypePhoBrang -->

    <owl:NamedIndividual rdf:about="http://purl.bdrc.io/resource/PlaceTypePhoBrang">
        <rdf:type rdf:resource="http://purl.bdrc.io/ontology/PlaceType"/>
    </owl:NamedIndividual>
    


    <!-- http://purl.bdrc.io/resource/PlaceTypePhu -->

    <owl:NamedIndividual rdf:about="http://purl.bdrc.io/resource/PlaceTypePhu">
        <rdf:type rdf:resource="http://purl.bdrc.io/ontology/PlaceType"/>
    </owl:NamedIndividual>
    


    <!-- http://purl.bdrc.io/resource/PlaceTypeRangByungKhorYug -->

    <owl:NamedIndividual rdf:about="http://purl.bdrc.io/resource/PlaceTypeRangByungKhorYug">
        <rdf:type rdf:resource="http://purl.bdrc.io/ontology/PlaceType"/>
        <rdfs:comment xml:lang="en">Natural features such as rivers, caves, mountain passes and so on</rdfs:comment>
        <rdfs:label xml:lang="en">Natural Features</rdfs:label>
        <rdfs:label xml:lang="bo-x-ewts">rang byung &apos;khor yug</rdfs:label>
        <rdfs:label xml:lang="zh">自然地域</rdfs:label>
    </owl:NamedIndividual>
    


    <!-- http://purl.bdrc.io/resource/PlaceTypeRangSkyongKhul -->

    <owl:NamedIndividual rdf:about="http://purl.bdrc.io/resource/PlaceTypeRangSkyongKhul">
        <rdf:type rdf:resource="http://purl.bdrc.io/ontology/PlaceType"/>
    </owl:NamedIndividual>
    


    <!-- http://purl.bdrc.io/resource/PlaceTypeRangSkyongLjongs -->

    <owl:NamedIndividual rdf:about="http://purl.bdrc.io/resource/PlaceTypeRangSkyongLjongs">
        <rdf:type rdf:resource="http://purl.bdrc.io/ontology/PlaceType"/>
    </owl:NamedIndividual>
    


    <!-- http://purl.bdrc.io/resource/PlaceTypeRdoRing -->

    <owl:NamedIndividual rdf:about="http://purl.bdrc.io/resource/PlaceTypeRdoRing">
        <rdf:type rdf:resource="http://purl.bdrc.io/ontology/PlaceType"/>
    </owl:NamedIndividual>
    


    <!-- http://purl.bdrc.io/resource/PlaceTypeRdzong -->

    <owl:NamedIndividual rdf:about="http://purl.bdrc.io/resource/PlaceTypeRdzong">
        <rdf:type rdf:resource="http://purl.bdrc.io/ontology/PlaceType"/>
    </owl:NamedIndividual>
    


    <!-- http://purl.bdrc.io/resource/PlaceTypeRgyalKhab -->

    <owl:NamedIndividual rdf:about="http://purl.bdrc.io/resource/PlaceTypeRgyalKhab">
        <rdf:type rdf:resource="http://purl.bdrc.io/ontology/PlaceType"/>
    </owl:NamedIndividual>
    


    <!-- http://purl.bdrc.io/resource/PlaceTypeRgyalPhran -->

    <owl:NamedIndividual rdf:about="http://purl.bdrc.io/resource/PlaceTypeRgyalPhran">
        <rdf:type rdf:resource="http://purl.bdrc.io/ontology/PlaceType"/>
    </owl:NamedIndividual>
    


    <!-- http://purl.bdrc.io/resource/PlaceTypeRiBo -->

    <owl:NamedIndividual rdf:about="http://purl.bdrc.io/resource/PlaceTypeRiBo">
        <rdf:type rdf:resource="http://purl.bdrc.io/ontology/PlaceType"/>
    </owl:NamedIndividual>
    


    <!-- http://purl.bdrc.io/resource/PlaceTypeRiKhrod -->

    <owl:NamedIndividual rdf:about="http://purl.bdrc.io/resource/PlaceTypeRiKhrod">
        <rdf:type rdf:resource="http://purl.bdrc.io/ontology/PlaceType"/>
    </owl:NamedIndividual>
    


    <!-- http://purl.bdrc.io/resource/PlaceTypeRiRgyud -->

    <owl:NamedIndividual rdf:about="http://purl.bdrc.io/resource/PlaceTypeRiRgyud">
        <rdf:type rdf:resource="http://purl.bdrc.io/ontology/PlaceType"/>
    </owl:NamedIndividual>
    


    <!-- http://purl.bdrc.io/resource/PlaceTypeRong -->

    <owl:NamedIndividual rdf:about="http://purl.bdrc.io/resource/PlaceTypeRong">
        <rdf:type rdf:resource="http://purl.bdrc.io/ontology/PlaceType"/>
    </owl:NamedIndividual>
    


    <!-- http://purl.bdrc.io/resource/PlaceTypeRtenGzhiYulLung -->

    <owl:NamedIndividual rdf:about="http://purl.bdrc.io/resource/PlaceTypeRtenGzhiYulLung">
        <rdf:type rdf:resource="http://purl.bdrc.io/ontology/PlaceType"/>
        <rdfs:comment xml:lang="en">Various kinds of semi-formal and historical references to extended geographic areas such as administrative districts, isolated areas, premodern counties and so on.</rdfs:comment>
        <rdfs:label xml:lang="en">Regions</rdfs:label>
        <rdfs:label xml:lang="bo-x-ewts">rten gzhi yul lung</rdfs:label>
        <rdfs:label xml:lang="zh">区域</rdfs:label>
    </owl:NamedIndividual>
    


    <!-- http://purl.bdrc.io/resource/PlaceTypeRu -->

    <owl:NamedIndividual rdf:about="http://purl.bdrc.io/resource/PlaceTypeRu">
        <rdf:type rdf:resource="http://purl.bdrc.io/ontology/PlaceType"/>
    </owl:NamedIndividual>
    


    <!-- http://purl.bdrc.io/resource/PlaceTypeRuSde -->

    <owl:NamedIndividual rdf:about="http://purl.bdrc.io/resource/PlaceTypeRuSde">
        <rdf:type rdf:resource="http://purl.bdrc.io/ontology/PlaceType"/>
    </owl:NamedIndividual>
    


    <!-- http://purl.bdrc.io/resource/PlaceTypeSaKhul -->

    <owl:NamedIndividual rdf:about="http://purl.bdrc.io/resource/PlaceTypeSaKhul">
        <rdf:type rdf:resource="http://purl.bdrc.io/ontology/PlaceType"/>
    </owl:NamedIndividual>
    


    <!-- http://purl.bdrc.io/resource/PlaceTypeSbasYul -->

    <owl:NamedIndividual rdf:about="http://purl.bdrc.io/resource/PlaceTypeSbasYul">
        <rdf:type rdf:resource="http://purl.bdrc.io/ontology/PlaceType"/>
    </owl:NamedIndividual>
    


    <!-- http://purl.bdrc.io/resource/PlaceTypeSdeDponMngaRis -->

    <owl:NamedIndividual rdf:about="http://purl.bdrc.io/resource/PlaceTypeSdeDponMngaRis">
        <rdf:type rdf:resource="http://purl.bdrc.io/ontology/PlaceType"/>
    </owl:NamedIndividual>
    


    <!-- http://purl.bdrc.io/resource/PlaceTypeSdeTsho -->

    <owl:NamedIndividual rdf:about="http://purl.bdrc.io/resource/PlaceTypeSdeTsho">
        <rdf:type rdf:resource="http://purl.bdrc.io/ontology/PlaceType"/>
    </owl:NamedIndividual>
    


    <!-- http://purl.bdrc.io/resource/PlaceTypeSgang -->

    <owl:NamedIndividual rdf:about="http://purl.bdrc.io/resource/PlaceTypeSgang">
        <rdf:type rdf:resource="http://purl.bdrc.io/ontology/PlaceType"/>
    </owl:NamedIndividual>
    


    <!-- http://purl.bdrc.io/resource/PlaceTypeSgrubGrwa -->

    <owl:NamedIndividual rdf:about="http://purl.bdrc.io/resource/PlaceTypeSgrubGrwa">
        <rdf:type rdf:resource="http://purl.bdrc.io/ontology/PlaceType"/>
    </owl:NamedIndividual>
    


    <!-- http://purl.bdrc.io/resource/PlaceTypeSgrubPhug -->

    <owl:NamedIndividual rdf:about="http://purl.bdrc.io/resource/PlaceTypeSgrubPhug">
        <rdf:type rdf:resource="http://purl.bdrc.io/ontology/PlaceType"/>
    </owl:NamedIndividual>
    


    <!-- http://purl.bdrc.io/resource/PlaceTypeShang -->

    <owl:NamedIndividual rdf:about="http://purl.bdrc.io/resource/PlaceTypeShang">
        <rdf:type rdf:resource="http://purl.bdrc.io/ontology/PlaceType"/>
    </owl:NamedIndividual>
    


    <!-- http://purl.bdrc.io/resource/PlaceTypeSkor -->

    <owl:NamedIndividual rdf:about="http://purl.bdrc.io/resource/PlaceTypeSkor">
        <rdf:type rdf:resource="http://purl.bdrc.io/ontology/PlaceType"/>
    </owl:NamedIndividual>
    


    <!-- http://purl.bdrc.io/resource/PlaceTypeSlobGrwa -->

    <owl:NamedIndividual rdf:about="http://purl.bdrc.io/resource/PlaceTypeSlobGrwa">
        <rdf:type rdf:resource="http://purl.bdrc.io/ontology/PlaceType"/>
    </owl:NamedIndividual>
    


    <!-- http://purl.bdrc.io/resource/PlaceTypeSmanKhang -->

    <owl:NamedIndividual rdf:about="http://purl.bdrc.io/resource/PlaceTypeSmanKhang">
        <rdf:type rdf:resource="http://purl.bdrc.io/ontology/PlaceType"/>
    </owl:NamedIndividual>
    


    <!-- http://purl.bdrc.io/resource/PlaceTypeSngarGyiRdzong -->

    <owl:NamedIndividual rdf:about="http://purl.bdrc.io/resource/PlaceTypeSngarGyiRdzong">
        <rdf:type rdf:resource="http://purl.bdrc.io/ontology/PlaceType"/>
    </owl:NamedIndividual>
    


    <!-- http://purl.bdrc.io/resource/PlaceTypeSrolRgyunGyiSaMing -->

    <owl:NamedIndividual rdf:about="http://purl.bdrc.io/resource/PlaceTypeSrolRgyunGyiSaMing">
        <rdf:type rdf:resource="http://purl.bdrc.io/ontology/PlaceType"/>
    </owl:NamedIndividual>
    


    <!-- http://purl.bdrc.io/resource/PlaceTypeSrolRgyunSaKhul -->

    <owl:NamedIndividual rdf:about="http://purl.bdrc.io/resource/PlaceTypeSrolRgyunSaKhul">
        <rdf:type rdf:resource="http://purl.bdrc.io/ontology/PlaceType"/>
    </owl:NamedIndividual>
    


    <!-- http://purl.bdrc.io/resource/PlaceTypeStongSde -->

    <owl:NamedIndividual rdf:about="http://purl.bdrc.io/resource/PlaceTypeStongSde">
        <rdf:type rdf:resource="http://purl.bdrc.io/ontology/PlaceType"/>
    </owl:NamedIndividual>
    


    <!-- http://purl.bdrc.io/resource/PlaceTypeThang -->

    <owl:NamedIndividual rdf:about="http://purl.bdrc.io/resource/PlaceTypeThang">
        <rdf:type rdf:resource="http://purl.bdrc.io/ontology/PlaceType"/>
    </owl:NamedIndividual>
    


    <!-- http://purl.bdrc.io/resource/PlaceTypeTshoBa -->

    <owl:NamedIndividual rdf:about="http://purl.bdrc.io/resource/PlaceTypeTshoBa">
        <rdf:type rdf:resource="http://purl.bdrc.io/ontology/PlaceType"/>
    </owl:NamedIndividual>
    


    <!-- http://purl.bdrc.io/resource/PlaceTypeTshongDus -->

    <owl:NamedIndividual rdf:about="http://purl.bdrc.io/resource/PlaceTypeTshongDus">
        <rdf:type rdf:resource="http://purl.bdrc.io/ontology/PlaceType"/>
    </owl:NamedIndividual>
    


    <!-- http://purl.bdrc.io/resource/PlaceTypeYulChen -->

    <owl:NamedIndividual rdf:about="http://purl.bdrc.io/resource/PlaceTypeYulChen">
        <rdf:type rdf:resource="http://purl.bdrc.io/ontology/PlaceType"/>
    </owl:NamedIndividual>
    


    <!-- http://purl.bdrc.io/resource/PlaceTypeYulPhran -->

    <owl:NamedIndividual rdf:about="http://purl.bdrc.io/resource/PlaceTypeYulPhran">
        <rdf:type rdf:resource="http://purl.bdrc.io/ontology/PlaceType"/>
    </owl:NamedIndividual>
    


    <!-- http://purl.bdrc.io/resource/PlaceTypeYulSde -->

    <owl:NamedIndividual rdf:about="http://purl.bdrc.io/resource/PlaceTypeYulSde">
        <rdf:type rdf:resource="http://purl.bdrc.io/ontology/PlaceType"/>
    </owl:NamedIndividual>
    


    <!-- http://purl.bdrc.io/resource/PlaceTypeZamPa -->

    <owl:NamedIndividual rdf:about="http://purl.bdrc.io/resource/PlaceTypeZamPa">
        <rdf:type rdf:resource="http://purl.bdrc.io/ontology/PlaceType"/>
    </owl:NamedIndividual>
    


    <!-- http://purl.bdrc.io/resource/PlaceTypeZhingChen -->

    <owl:NamedIndividual rdf:about="http://purl.bdrc.io/resource/PlaceTypeZhingChen">
        <rdf:type rdf:resource="http://purl.bdrc.io/ontology/PlaceType"/>
    </owl:NamedIndividual>
    


    <!-- http://purl.bdrc.io/resource/PrintTypeBlockPrint -->

    <owl:NamedIndividual rdf:about="http://purl.bdrc.io/resource/PrintTypeBlockPrint">
        <rdf:type rdf:resource="http://purl.bdrc.io/ontology/PrintType"/>
    </owl:NamedIndividual>
    


    <!-- http://purl.bdrc.io/resource/PrintTypeComputerInput -->

    <owl:NamedIndividual rdf:about="http://purl.bdrc.io/resource/PrintTypeComputerInput">
        <rdf:type rdf:resource="http://purl.bdrc.io/ontology/PrintType"/>
    </owl:NamedIndividual>
    


    <!-- http://purl.bdrc.io/resource/PrintTypeDbuCan -->

    <owl:NamedIndividual rdf:about="http://purl.bdrc.io/resource/PrintTypeDbuCan">
        <rdf:type rdf:resource="http://purl.bdrc.io/ontology/PrintType"/>
    </owl:NamedIndividual>
    


    <!-- http://purl.bdrc.io/resource/PrintTypeDbuMed -->

    <owl:NamedIndividual rdf:about="http://purl.bdrc.io/resource/PrintTypeDbuMed">
        <rdf:type rdf:resource="http://purl.bdrc.io/ontology/PrintType"/>
    </owl:NamedIndividual>
    


    <!-- http://purl.bdrc.io/resource/PrintTypeFacsimile -->

    <owl:NamedIndividual rdf:about="http://purl.bdrc.io/resource/PrintTypeFacsimile">
        <rdf:type rdf:resource="http://purl.bdrc.io/ontology/PrintType"/>
    </owl:NamedIndividual>
    


    <!-- http://purl.bdrc.io/resource/PrintTypeOCR -->

    <owl:NamedIndividual rdf:about="http://purl.bdrc.io/resource/PrintTypeOCR">
        <rdf:type rdf:resource="http://purl.bdrc.io/ontology/PrintType"/>
    </owl:NamedIndividual>
    


    <!-- http://purl.bdrc.io/resource/PrintTypeTypeSet -->

    <owl:NamedIndividual rdf:about="http://purl.bdrc.io/resource/PrintTypeTypeSet">
        <rdf:type rdf:resource="http://purl.bdrc.io/ontology/PrintType"/>
    </owl:NamedIndividual>
    


    <!-- http://purl.bdrc.io/resource/StatusAccessioned -->

    <owl:NamedIndividual rdf:about="http://purl.bdrc.io/resource/StatusAccessioned">
        <rdf:type rdf:resource="http://purl.bdrc.io/ontology/StatusType"/>
        <rdfs:label xml:lang="en">accessioned</rdfs:label>
    </owl:NamedIndividual>
    


    <!-- http://purl.bdrc.io/resource/StatusAcquiring -->

    <owl:NamedIndividual rdf:about="http://purl.bdrc.io/resource/StatusAcquiring">
        <rdf:type rdf:resource="http://purl.bdrc.io/ontology/StatusType"/>
        <rdfs:label xml:lang="en">acquiring</rdfs:label>
    </owl:NamedIndividual>
    


    <!-- http://purl.bdrc.io/resource/StatusEditing -->

    <owl:NamedIndividual rdf:about="http://purl.bdrc.io/resource/StatusEditing">
        <rdf:type rdf:resource="http://purl.bdrc.io/ontology/StatusType"/>
        <rdfs:label xml:lang="en">editing</rdfs:label>
    </owl:NamedIndividual>
    


    <!-- http://purl.bdrc.io/resource/StatusOnHold -->

    <owl:NamedIndividual rdf:about="http://purl.bdrc.io/resource/StatusOnHold">
        <rdf:type rdf:resource="http://purl.bdrc.io/ontology/StatusType"/>
        <rdfs:label xml:lang="en">on hold</rdfs:label>
    </owl:NamedIndividual>
    


    <!-- http://purl.bdrc.io/resource/StatusProvisional -->

    <owl:NamedIndividual rdf:about="http://purl.bdrc.io/resource/StatusProvisional">
        <rdf:type rdf:resource="http://purl.bdrc.io/ontology/StatusType"/>
        <rdfs:label xml:lang="en">provisional</rdfs:label>
    </owl:NamedIndividual>
    


    <!-- http://purl.bdrc.io/resource/StatusReleased -->

    <owl:NamedIndividual rdf:about="http://purl.bdrc.io/resource/StatusReleased">
        <rdf:type rdf:resource="http://purl.bdrc.io/ontology/StatusType"/>
        <rdfs:label xml:lang="en">released</rdfs:label>
    </owl:NamedIndividual>
    


    <!-- http://purl.bdrc.io/resource/StatusScanned -->

    <owl:NamedIndividual rdf:about="http://purl.bdrc.io/resource/StatusScanned">
        <rdf:type rdf:resource="http://purl.bdrc.io/ontology/StatusType"/>
        <rdfs:label xml:lang="en">scanned</rdfs:label>
    </owl:NamedIndividual>
    


    <!-- http://purl.bdrc.io/resource/StatusSeekingOut -->

    <owl:NamedIndividual rdf:about="http://purl.bdrc.io/resource/StatusSeekingOut">
        <rdf:type rdf:resource="http://purl.bdrc.io/ontology/StatusType"/>
        <rdfs:label xml:lang="en">seeking out</rdfs:label>
    </owl:NamedIndividual>
    


    <!-- http://purl.bdrc.io/resource/StatusWithdrawn -->

    <owl:NamedIndividual rdf:about="http://purl.bdrc.io/resource/StatusWithdrawn">
        <rdf:type rdf:resource="http://purl.bdrc.io/ontology/StatusType"/>
        <rdfs:label xml:lang="en">withdrawn</rdfs:label>
    </owl:NamedIndividual>
    


    <!-- http://purl.bdrc.io/resource/TraditionBaromKagyu -->

    <owl:NamedIndividual rdf:about="http://purl.bdrc.io/resource/TraditionBaromKagyu">
        <rdf:type rdf:resource="http://purl.bdrc.io/ontology/Tradition"/>
    </owl:NamedIndividual>
    


    <!-- http://purl.bdrc.io/resource/TraditionBodong -->

    <owl:NamedIndividual rdf:about="http://purl.bdrc.io/resource/TraditionBodong">
        <rdf:type rdf:resource="http://purl.bdrc.io/ontology/Tradition"/>
    </owl:NamedIndividual>
    


    <!-- http://purl.bdrc.io/resource/TraditionBon -->

    <owl:NamedIndividual rdf:about="http://purl.bdrc.io/resource/TraditionBon">
        <rdf:type rdf:resource="http://purl.bdrc.io/ontology/Tradition"/>
    </owl:NamedIndividual>
    


    <!-- http://purl.bdrc.io/resource/TraditionChod -->

    <owl:NamedIndividual rdf:about="http://purl.bdrc.io/resource/TraditionChod">
        <rdf:type rdf:resource="http://purl.bdrc.io/ontology/Tradition"/>
    </owl:NamedIndividual>
    


    <!-- http://purl.bdrc.io/resource/TraditionDrigungKagyu -->

    <owl:NamedIndividual rdf:about="http://purl.bdrc.io/resource/TraditionDrigungKagyu">
        <rdf:type rdf:resource="http://purl.bdrc.io/ontology/Tradition"/>
    </owl:NamedIndividual>
    


    <!-- http://purl.bdrc.io/resource/TraditionDrukpaKagyu -->

    <owl:NamedIndividual rdf:about="http://purl.bdrc.io/resource/TraditionDrukpaKagyu">
        <rdf:type rdf:resource="http://purl.bdrc.io/ontology/Tradition"/>
    </owl:NamedIndividual>
    


    <!-- http://purl.bdrc.io/resource/TraditionGeluk -->

    <owl:NamedIndividual rdf:about="http://purl.bdrc.io/resource/TraditionGeluk">
        <rdf:type rdf:resource="http://purl.bdrc.io/ontology/Tradition"/>
    </owl:NamedIndividual>
    


    <!-- http://purl.bdrc.io/resource/TraditionJonang -->

    <owl:NamedIndividual rdf:about="http://purl.bdrc.io/resource/TraditionJonang">
        <rdf:type rdf:resource="http://purl.bdrc.io/ontology/Tradition"/>
    </owl:NamedIndividual>
    


    <!-- http://purl.bdrc.io/resource/TraditionKadam -->

    <owl:NamedIndividual rdf:about="http://purl.bdrc.io/resource/TraditionKadam">
        <rdf:type rdf:resource="http://purl.bdrc.io/ontology/Tradition"/>
    </owl:NamedIndividual>
    


    <!-- http://purl.bdrc.io/resource/TraditionKagyu -->

    <owl:NamedIndividual rdf:about="http://purl.bdrc.io/resource/TraditionKagyu">
        <rdf:type rdf:resource="http://purl.bdrc.io/ontology/Tradition"/>
    </owl:NamedIndividual>
    


    <!-- http://purl.bdrc.io/resource/TraditionKarmaKagyu -->

    <owl:NamedIndividual rdf:about="http://purl.bdrc.io/resource/TraditionKarmaKagyu">
        <rdf:type rdf:resource="http://purl.bdrc.io/ontology/Tradition"/>
    </owl:NamedIndividual>
    


    <!-- http://purl.bdrc.io/resource/TraditionMarpaKagyu -->

    <owl:NamedIndividual rdf:about="http://purl.bdrc.io/resource/TraditionMarpaKagyu">
        <rdf:type rdf:resource="http://purl.bdrc.io/ontology/Tradition"/>
    </owl:NamedIndividual>
    


    <!-- http://purl.bdrc.io/resource/TraditionNedoKagyu -->

    <owl:NamedIndividual rdf:about="http://purl.bdrc.io/resource/TraditionNedoKagyu">
        <rdf:type rdf:resource="http://purl.bdrc.io/ontology/Tradition"/>
    </owl:NamedIndividual>
    


    <!-- http://purl.bdrc.io/resource/TraditionNgorSakya -->

    <owl:NamedIndividual rdf:about="http://purl.bdrc.io/resource/TraditionNgorSakya">
        <rdf:type rdf:resource="http://purl.bdrc.io/ontology/Tradition"/>
    </owl:NamedIndividual>
    


    <!-- http://purl.bdrc.io/resource/TraditionNyingma -->

    <owl:NamedIndividual rdf:about="http://purl.bdrc.io/resource/TraditionNyingma">
        <rdf:type rdf:resource="http://purl.bdrc.io/ontology/Tradition"/>
    </owl:NamedIndividual>
    


    <!-- http://purl.bdrc.io/resource/TraditionRime -->

    <owl:NamedIndividual rdf:about="http://purl.bdrc.io/resource/TraditionRime">
        <rdf:type rdf:resource="http://purl.bdrc.io/ontology/Tradition"/>
    </owl:NamedIndividual>
    


    <!-- http://purl.bdrc.io/resource/TraditionSakya -->

    <owl:NamedIndividual rdf:about="http://purl.bdrc.io/resource/TraditionSakya">
        <rdf:type rdf:resource="http://purl.bdrc.io/ontology/Tradition"/>
    </owl:NamedIndividual>
    


    <!-- http://purl.bdrc.io/resource/TraditionShangpaKagyu -->

    <owl:NamedIndividual rdf:about="http://purl.bdrc.io/resource/TraditionShangpaKagyu">
        <rdf:type rdf:resource="http://purl.bdrc.io/ontology/Tradition"/>
    </owl:NamedIndividual>
    


    <!-- http://purl.bdrc.io/resource/TraditionTaklungKagyu -->

    <owl:NamedIndividual rdf:about="http://purl.bdrc.io/resource/TraditionTaklungKagyu">
        <rdf:type rdf:resource="http://purl.bdrc.io/ontology/Tradition"/>
    </owl:NamedIndividual>
    


    <!-- http://purl.bdrc.io/resource/TraditionTodrukKagyu -->

    <owl:NamedIndividual rdf:about="http://purl.bdrc.io/resource/TraditionTodrukKagyu">
        <rdf:type rdf:resource="http://purl.bdrc.io/ontology/Tradition"/>
    </owl:NamedIndividual>
    


    <!-- http://purl.bdrc.io/resource/TraditionTsalpaKagyu -->

    <owl:NamedIndividual rdf:about="http://purl.bdrc.io/resource/TraditionTsalpaKagyu">
        <rdf:type rdf:resource="http://purl.bdrc.io/ontology/Tradition"/>
    </owl:NamedIndividual>
    


    <!-- http://purl.bdrc.io/resource/TraditionYazangKagyu -->

    <owl:NamedIndividual rdf:about="http://purl.bdrc.io/resource/TraditionYazangKagyu">
        <rdf:type rdf:resource="http://purl.bdrc.io/ontology/Tradition"/>
    </owl:NamedIndividual>
    


    <!-- http://purl.bdrc.io/resource/TraditionYelpaKagyu -->

    <owl:NamedIndividual rdf:about="http://purl.bdrc.io/resource/TraditionYelpaKagyu">
        <rdf:type rdf:resource="http://purl.bdrc.io/ontology/Tradition"/>
    </owl:NamedIndividual>
    


    <!-- http://purl.bdrc.io/resource/TraditionZhalu -->

    <owl:NamedIndividual rdf:about="http://purl.bdrc.io/resource/TraditionZhalu">
        <rdf:type rdf:resource="http://purl.bdrc.io/ontology/Tradition"/>
    </owl:NamedIndividual>
    


    <!-- http://purl.bdrc.io/resource/TraditionZhije -->

    <owl:NamedIndividual rdf:about="http://purl.bdrc.io/resource/TraditionZhije">
        <rdf:type rdf:resource="http://purl.bdrc.io/ontology/Tradition"/>
    </owl:NamedIndividual>
    


    <!-- http://purl.bdrc.io/resource/TraditionZurmangKagyu -->

    <owl:NamedIndividual rdf:about="http://purl.bdrc.io/resource/TraditionZurmangKagyu">
        <rdf:type rdf:resource="http://purl.bdrc.io/ontology/Tradition"/>
    </owl:NamedIndividual>
    


    <!-- http://purl.bdrc.io/resource/UNKNOWN_Corporation -->

    <owl:NamedIndividual rdf:about="http://purl.bdrc.io/resource/UNKNOWN_Corporation">
        <rdf:type rdf:resource="http://purl.bdrc.io/ontology/Corporation"/>
        <status rdf:resource="http://purl.bdrc.io/resource/StatusReleased"/>
        <rdfs:isDefinedBy rdf:resource="http://purl.bdrc.io/data/UNKNOWN_Corporation"/>
        <rdfs:label xml:lang="en">Unkown</rdfs:label>
    </owl:NamedIndividual>
    


    <!-- http://purl.bdrc.io/resource/UNKNOWN_Lineage -->

    <owl:NamedIndividual rdf:about="http://purl.bdrc.io/resource/UNKNOWN_Lineage">
        <rdf:type rdf:resource="http://purl.bdrc.io/ontology/Lineage"/>
        <status rdf:resource="http://purl.bdrc.io/resource/StatusReleased"/>
        <rdfs:isDefinedBy rdf:resource="http://purl.bdrc.io/data/UNKNOWN_Lineage"/>
        <rdfs:label xml:lang="en">Unknown</rdfs:label>
    </owl:NamedIndividual>
    


    <!-- http://purl.bdrc.io/resource/UNKNOWN_Person -->

    <owl:NamedIndividual rdf:about="http://purl.bdrc.io/resource/UNKNOWN_Person">
        <rdf:type rdf:resource="http://purl.bdrc.io/ontology/Person"/>
        <status rdf:resource="http://purl.bdrc.io/resource/StatusReleased"/>
        <rdfs:isDefinedBy rdf:resource="http://purl.bdrc.io/data/UNKNOWN_Person"/>
        <rdfs:label xml:lang="en">Unknown</rdfs:label>
    </owl:NamedIndividual>
    


    <!-- http://purl.bdrc.io/resource/UNKNOWN_Place -->

    <owl:NamedIndividual rdf:about="http://purl.bdrc.io/resource/UNKNOWN_Place">
        <rdf:type rdf:resource="http://purl.bdrc.io/ontology/Place"/>
        <status rdf:resource="http://purl.bdrc.io/resource/StatusReleased"/>
        <rdfs:isDefinedBy rdf:resource="http://purl.bdrc.io/data/UNKNOWN_Place"/>
        <rdfs:label xml:lang="en">Unknown</rdfs:label>
    </owl:NamedIndividual>
    


    <!-- http://purl.bdrc.io/resource/UNKNOWN_Product -->

    <owl:NamedIndividual rdf:about="http://purl.bdrc.io/resource/UNKNOWN_Product">
        <rdf:type rdf:resource="http://purl.bdrc.io/ontology/admin/Product"/>
        <status rdf:resource="http://purl.bdrc.io/resource/StatusReleased"/>
        <rdfs:isDefinedBy rdf:resource="http://purl.bdrc.io/data/UNKNOWN_Product"/>
        <rdfs:label xml:lang="en">Unknown</rdfs:label>
    </owl:NamedIndividual>
    


    <!-- http://purl.bdrc.io/resource/UNKNOWN_Role -->

    <owl:NamedIndividual rdf:about="http://purl.bdrc.io/resource/UNKNOWN_Role">
        <rdf:type rdf:resource="http://purl.bdrc.io/ontology/Role"/>
        <status rdf:resource="http://purl.bdrc.io/resource/StatusReleased"/>
        <rdfs:isDefinedBy rdf:resource="http://purl.bdrc.io/data/UNKNOWN_Role"/>
        <rdfs:label xml:lang="en">Unknown</rdfs:label>
    </owl:NamedIndividual>
    


    <!-- http://purl.bdrc.io/resource/UNKNOWN_Topic -->

    <owl:NamedIndividual rdf:about="http://purl.bdrc.io/resource/UNKNOWN_Topic">
        <rdf:type rdf:resource="http://purl.bdrc.io/ontology/Topic"/>
        <status rdf:resource="http://purl.bdrc.io/resource/StatusReleased"/>
        <rdfs:isDefinedBy rdf:resource="http://purl.bdrc.io/data/UNKNOWN_Topic"/>
        <rdfs:label xml:lang="en">Unknown</rdfs:label>
    </owl:NamedIndividual>
    


    <!-- http://purl.bdrc.io/resource/UNKNOWN_Work -->

    <owl:NamedIndividual rdf:about="http://purl.bdrc.io/resource/UNKNOWN_Work">
        <rdf:type rdf:resource="http://purl.bdrc.io/ontology/Work"/>
        <status rdf:resource="http://purl.bdrc.io/resource/StatusReleased"/>
        <rdfs:isDefinedBy rdf:resource="http://purl.bdrc.io/data/UNKNOWN_Work"/>
        <rdfs:label xml:lang="en">Unknown</rdfs:label>
    </owl:NamedIndividual>
    


    <!-- http://purl.bdrc.io/resource/WorkAccessFairUse -->

    <owl:NamedIndividual rdf:about="http://purl.bdrc.io/resource/WorkAccessFairUse">
        <rdf:type rdf:resource="http://purl.bdrc.io/ontology/WorkAccessType"/>
        <rdfs:comment xml:lang="en">A copyrighted Work permits a small portion of its contents to be made available</rdfs:comment>
        <rdfs:label xml:lang="en">Fair Use</rdfs:label>
    </owl:NamedIndividual>
    


    <!-- http://purl.bdrc.io/resource/WorkAccessOpen -->

    <owl:NamedIndividual rdf:about="http://purl.bdrc.io/resource/WorkAccessOpen">
        <rdf:type rdf:resource="http://purl.bdrc.io/ontology/WorkAccessType"/>
        <rdfs:comment xml:lang="en">The contents of the Work are freely avaiable in their entirety</rdfs:comment>
        <rdfs:label xml:lang="en">Open Access</rdfs:label>
    </owl:NamedIndividual>
    


    <!-- http://purl.bdrc.io/resource/WorkAccessRestrictedByQuality -->

    <owl:NamedIndividual rdf:about="http://purl.bdrc.io/resource/WorkAccessRestrictedByQuality">
        <rdf:type rdf:resource="http://purl.bdrc.io/ontology/WorkAccessType"/>
        <rdfs:comment xml:lang="en">The quality of the scanning or eText conversion to poor to warrant making it available online.</rdfs:comment>
        <rdfs:label xml:lang="en">Restricted by Quality</rdfs:label>
    </owl:NamedIndividual>
    


    <!-- http://purl.bdrc.io/resource/WorkAccessRestrictedByTbrc -->

    <owl:NamedIndividual rdf:about="http://purl.bdrc.io/resource/WorkAccessRestrictedByTbrc">
        <rdf:type rdf:resource="http://purl.bdrc.io/ontology/WorkAccessType"/>
        <rdfs:comment xml:lang="en">BDRC is restricting access to the Work.</rdfs:comment>
        <rdfs:label xml:lang="en">Restricted by BDRC</rdfs:label>
    </owl:NamedIndividual>
    


    <!-- http://purl.bdrc.io/resource/WorkAccessRestrictedInChina -->

    <owl:NamedIndividual rdf:about="http://purl.bdrc.io/resource/WorkAccessRestrictedInChina">
        <rdf:type rdf:resource="http://purl.bdrc.io/ontology/WorkAccessType"/>
        <rdfs:comment xml:lang="en">The Work is not to be made available in the PRC.</rdfs:comment>
        <rdfs:label xml:lang="en">Restricted in China</rdfs:label>
    </owl:NamedIndividual>
    


    <!-- http://purl.bdrc.io/resource/WorkAccessRestrictedSealed -->

    <owl:NamedIndividual rdf:about="http://purl.bdrc.io/resource/WorkAccessRestrictedSealed">
        <rdf:type rdf:resource="http://purl.bdrc.io/ontology/WorkAccessType"/>
        <rdfs:comment xml:lang="en">The Work is sealed by tradition.</rdfs:comment>
        <rdfs:label xml:lang="en">Restricted Sealed</rdfs:label>
    </owl:NamedIndividual>
    


    <!-- http://purl.bdrc.io/resource/WorkAccessRestrictedTemporarily -->

    <owl:NamedIndividual rdf:about="http://purl.bdrc.io/resource/WorkAccessRestrictedTemporarily">
        <rdf:type rdf:resource="http://purl.bdrc.io/ontology/WorkAccessType"/>
        <rdfs:comment xml:lang="en">The Work is temporarily restricted.</rdfs:comment>
        <rdfs:label xml:lang="en">Temporarily Restricted</rdfs:label>
    </owl:NamedIndividual>
    


    <!-- http://purl.bdrc.io/resource/WorkBibliographicTitle -->

    <owl:NamedIndividual rdf:about="http://purl.bdrc.io/resource/WorkBibliographicTitle">
        <rdf:type rdf:resource="http://purl.bdrc.io/ontology/WorkTitleType"/>
    </owl:NamedIndividual>
    


    <!-- http://purl.bdrc.io/resource/WorkCaptionTitle -->

    <owl:NamedIndividual rdf:about="http://purl.bdrc.io/resource/WorkCaptionTitle">
        <rdf:type rdf:resource="http://purl.bdrc.io/ontology/WorkTitleType"/>
    </owl:NamedIndividual>
    


    <!-- http://purl.bdrc.io/resource/WorkChapter -->

    <owl:NamedIndividual rdf:about="http://purl.bdrc.io/resource/WorkChapter">
        <rdf:type rdf:resource="http://purl.bdrc.io/ontology/WorkPartType"/>
    </owl:NamedIndividual>
    


    <!-- http://purl.bdrc.io/resource/WorkColophonTitle -->

    <owl:NamedIndividual rdf:about="http://purl.bdrc.io/resource/WorkColophonTitle">
        <rdf:type rdf:resource="http://purl.bdrc.io/ontology/WorkTitleType"/>
    </owl:NamedIndividual>
    


    <!-- http://purl.bdrc.io/resource/WorkCopyrightPageTitle -->

    <owl:NamedIndividual rdf:about="http://purl.bdrc.io/resource/WorkCopyrightPageTitle">
        <rdf:type rdf:resource="http://purl.bdrc.io/ontology/WorkTitleType"/>
    </owl:NamedIndividual>
    


    <!-- http://purl.bdrc.io/resource/WorkCoverTitle -->

    <owl:NamedIndividual rdf:about="http://purl.bdrc.io/resource/WorkCoverTitle">
        <rdf:type rdf:resource="http://purl.bdrc.io/ontology/WorkTitleType"/>
    </owl:NamedIndividual>
    


    <!-- http://purl.bdrc.io/resource/WorkDkarChagTitle -->

    <owl:NamedIndividual rdf:about="http://purl.bdrc.io/resource/WorkDkarChagTitle">
        <rdf:type rdf:resource="http://purl.bdrc.io/ontology/WorkTitleType"/>
    </owl:NamedIndividual>
    


    <!-- http://purl.bdrc.io/resource/WorkFullTitle -->

    <owl:NamedIndividual rdf:about="http://purl.bdrc.io/resource/WorkFullTitle">
        <rdf:type rdf:resource="http://purl.bdrc.io/ontology/WorkTitleType"/>
    </owl:NamedIndividual>
    


    <!-- http://purl.bdrc.io/resource/WorkHalfTitle -->

    <owl:NamedIndividual rdf:about="http://purl.bdrc.io/resource/WorkHalfTitle">
        <rdf:type rdf:resource="http://purl.bdrc.io/ontology/WorkTitleType"/>
    </owl:NamedIndividual>
    


    <!-- http://purl.bdrc.io/resource/WorkIncipit -->

    <owl:NamedIndividual rdf:about="http://purl.bdrc.io/resource/WorkIncipit">
        <rdf:type rdf:resource="http://purl.bdrc.io/ontology/WorkTitleType"/>
    </owl:NamedIndividual>
    


    <!-- http://purl.bdrc.io/resource/WorkLicenseCCBY -->

    <owl:NamedIndividual rdf:about="http://purl.bdrc.io/resource/WorkLicenseCCBY">
        <rdf:type rdf:resource="http://purl.bdrc.io/ontology/WorkLicense"/>
        <rdfs:label xml:lang="en">CC-BY</rdfs:label>
        <rdfs:label xml:lang="en">The work is made available under Creative Commons, CC-BY, license with attribution</rdfs:label>
        <rdfs:seeAlso rdf:resource="http://creativecommons.org/licenses/"/>
    </owl:NamedIndividual>
    


    <!-- http://purl.bdrc.io/resource/WorkLicenseCopyrighted -->

    <owl:NamedIndividual rdf:about="http://purl.bdrc.io/resource/WorkLicenseCopyrighted">
        <rdf:type rdf:resource="http://purl.bdrc.io/ontology/WorkLicense"/>
        <rdfs:comment xml:lang="en">This work is copyrighted and BDRC will only make at most fairuse access available</rdfs:comment>
        <rdfs:label xml:lang="en">copyrighted</rdfs:label>
    </owl:NamedIndividual>
    


    <!-- http://purl.bdrc.io/resource/WorkLocationBegins -->

    <owl:NamedIndividual rdf:about="http://purl.bdrc.io/resource/WorkLocationBegins">
        <rdf:type rdf:resource="http://purl.bdrc.io/ontology/WorkLocationType"/>
        <rdfs:label xml:lang="en">Work Beginning</rdfs:label>
    </owl:NamedIndividual>
    


    <!-- http://purl.bdrc.io/resource/WorkLocationEnds -->

    <owl:NamedIndividual rdf:about="http://purl.bdrc.io/resource/WorkLocationEnds">
        <rdf:type rdf:resource="http://purl.bdrc.io/ontology/WorkLocationType"/>
        <rdfs:label xml:lang="en">Work Ending</rdfs:label>
    </owl:NamedIndividual>
    


    <!-- http://purl.bdrc.io/resource/WorkOtherTitle -->

    <owl:NamedIndividual rdf:about="http://purl.bdrc.io/resource/WorkOtherTitle">
        <rdf:type rdf:resource="http://purl.bdrc.io/ontology/WorkTitleType"/>
    </owl:NamedIndividual>
    


    <!-- http://purl.bdrc.io/resource/WorkRunningTitle -->

    <owl:NamedIndividual rdf:about="http://purl.bdrc.io/resource/WorkRunningTitle">
        <rdf:type rdf:resource="http://purl.bdrc.io/ontology/WorkTitleType"/>
    </owl:NamedIndividual>
    


    <!-- http://purl.bdrc.io/resource/WorkSection -->

    <owl:NamedIndividual rdf:about="http://purl.bdrc.io/resource/WorkSection">
        <rdf:type rdf:resource="http://purl.bdrc.io/ontology/WorkPartType"/>
    </owl:NamedIndividual>
    


    <!-- http://purl.bdrc.io/resource/WorkSectionTitle -->

    <owl:NamedIndividual rdf:about="http://purl.bdrc.io/resource/WorkSectionTitle">
        <rdf:type rdf:resource="http://purl.bdrc.io/ontology/WorkTitleType"/>
    </owl:NamedIndividual>
    


    <!-- http://purl.bdrc.io/resource/WorkSiteTypeCompleted -->

    <owl:NamedIndividual rdf:about="http://purl.bdrc.io/resource/WorkSiteTypeCompleted">
        <rdf:type rdf:resource="http://purl.bdrc.io/ontology/WorkSiteType"/>
    </owl:NamedIndividual>
    


    <!-- http://purl.bdrc.io/resource/WorkSiteTypeEdited -->

    <owl:NamedIndividual rdf:about="http://purl.bdrc.io/resource/WorkSiteTypeEdited">
        <rdf:type rdf:resource="http://purl.bdrc.io/ontology/WorkSiteType"/>
    </owl:NamedIndividual>
    


    <!-- http://purl.bdrc.io/resource/WorkSiteTypePrinted -->

    <owl:NamedIndividual rdf:about="http://purl.bdrc.io/resource/WorkSiteTypePrinted">
        <rdf:type rdf:resource="http://purl.bdrc.io/ontology/WorkSiteType"/>
    </owl:NamedIndividual>
    


    <!-- http://purl.bdrc.io/resource/WorkSiteTypeRevealed -->

    <owl:NamedIndividual rdf:about="http://purl.bdrc.io/resource/WorkSiteTypeRevealed">
        <rdf:type rdf:resource="http://purl.bdrc.io/ontology/WorkSiteType"/>
    </owl:NamedIndividual>
    


    <!-- http://purl.bdrc.io/resource/WorkSiteTypeStarted -->

    <owl:NamedIndividual rdf:about="http://purl.bdrc.io/resource/WorkSiteTypeStarted">
        <rdf:type rdf:resource="http://purl.bdrc.io/ontology/WorkSiteType"/>
    </owl:NamedIndividual>
    


    <!-- http://purl.bdrc.io/resource/WorkSiteTypeWritten -->

    <owl:NamedIndividual rdf:about="http://purl.bdrc.io/resource/WorkSiteTypeWritten">
        <rdf:type rdf:resource="http://purl.bdrc.io/ontology/WorkSiteType"/>
    </owl:NamedIndividual>
    


    <!-- http://purl.bdrc.io/resource/WorkSpineTitle -->

    <owl:NamedIndividual rdf:about="http://purl.bdrc.io/resource/WorkSpineTitle">
        <rdf:type rdf:resource="http://purl.bdrc.io/ontology/WorkTitleType"/>
    </owl:NamedIndividual>
    


    <!-- http://purl.bdrc.io/resource/WorkSubtitle -->

    <owl:NamedIndividual rdf:about="http://purl.bdrc.io/resource/WorkSubtitle">
        <rdf:type rdf:resource="http://purl.bdrc.io/ontology/WorkTitleType"/>
    </owl:NamedIndividual>
    


    <!-- http://purl.bdrc.io/resource/WorkText -->

    <owl:NamedIndividual rdf:about="http://purl.bdrc.io/resource/WorkText">
        <rdf:type rdf:resource="http://purl.bdrc.io/ontology/WorkPartType"/>
    </owl:NamedIndividual>
    


    <!-- http://purl.bdrc.io/resource/WorkTitlePageTitle -->

    <owl:NamedIndividual rdf:about="http://purl.bdrc.io/resource/WorkTitlePageTitle">
        <rdf:type rdf:resource="http://purl.bdrc.io/ontology/WorkTitleType"/>
    </owl:NamedIndividual>
    


    <!-- http://purl.bdrc.io/resource/WorkTitlePortion -->

    <owl:NamedIndividual rdf:about="http://purl.bdrc.io/resource/WorkTitlePortion">
        <rdf:type rdf:resource="http://purl.bdrc.io/ontology/WorkTitleType"/>
    </owl:NamedIndividual>
    


    <!-- http://purl.bdrc.io/resource/WorkTypeConceptualWork -->

    <owl:NamedIndividual rdf:about="http://purl.bdrc.io/resource/WorkTypeConceptualWork">
        <rdf:type rdf:resource="http://purl.bdrc.io/ontology/WorkType"/>
    </owl:NamedIndividual>
    


    <!-- http://purl.bdrc.io/resource/WorkTypePublishedWork -->

    <owl:NamedIndividual rdf:about="http://purl.bdrc.io/resource/WorkTypePublishedWork">
        <rdf:type rdf:resource="http://purl.bdrc.io/ontology/WorkType"/>
    </owl:NamedIndividual>
    


    <!-- http://purl.bdrc.io/resource/WorkTypeSeries -->

    <owl:NamedIndividual rdf:about="http://purl.bdrc.io/resource/WorkTypeSeries">
        <rdf:type rdf:resource="http://purl.bdrc.io/ontology/WorkType"/>
    </owl:NamedIndividual>
    


    <!-- http://purl.bdrc.io/resource/WorkTypeUnicodeText -->

    <owl:NamedIndividual rdf:about="http://purl.bdrc.io/resource/WorkTypeUnicodeText">
        <rdf:type rdf:resource="http://purl.bdrc.io/ontology/WorkType"/>
    </owl:NamedIndividual>
    


    <!-- http://purl.bdrc.io/resource/WorkVolume -->

    <owl:NamedIndividual rdf:about="http://purl.bdrc.io/resource/WorkVolume">
        <rdf:type rdf:resource="http://purl.bdrc.io/ontology/WorkPartType"/>
    </owl:NamedIndividual>
    


    <!-- 
    ///////////////////////////////////////////////////////////////////////////////////////
    //
    // Annotations
    //
    ///////////////////////////////////////////////////////////////////////////////////////
     -->

    <rdf:Description rdf:about="http://purl.bdrc.io/ontology/StatusType">
        <rdfs:label xml:lang="en">status</rdfs:label>
        <rdfs:comment xml:lang="en">Indicates the status of the subject description</rdfs:comment>
    </rdf:Description>
</rdf:RDF>



<!-- Generated by the OWL API (version 4.2.8.20170104-2310) https://github.com/owlcs/owlapi -->

