@prefix rdf: <http://www.w3.org/1999/02/22-rdf-syntax-ns#> .
@prefix dc: <http://purl.org/dc/elements/1.1/> .
@prefix foaf: <http://xmlns.com/foaf/0.1/> .
@prefix rdakit: <http://metadataregistry.org/uri/profile/rdakit/> .
@prefix rdfs: <http://www.w3.org/2000/01/rdf-schema#> .
@prefix reg: <http://metadataregistry.org/uri/profile/regap/> .
@prefix skos: <http://www.w3.org/2004/02/skos/core#> .

<http://metadataregistry.org/uri/RegStatus/1001>
    a skos:Concept ;
    skos:prefLabel "Published"@en .

<http://metadataregistry.org/uri/RegStatus/1008>
    a skos:Concept ;
    skos:prefLabel "Deprecated"@en .

<http://rdaregistry.info/Elements/e/>
    dc:title "RDA Expression properties"@en ;
    skos:note "Properties derived from RDA elements and relationship designators with the domain of RDA Expression."@en ;
    foaf:homepage <http://www.rdaregistry.info/Elements/e/> .

<http://rdaregistry.info/Elements/e/P20001>
    rdakit:instructionNumber "6.9" ;
    rdakit:toolkitDefinition "A categorization reflecting the fundamental form of communication in which the content is expressed and the human sense through which it is intended to be perceived."@en, "Catégorisation reflétant la forme fondamentale de communication sous laquelle le contenu est exprimé et le sens humain par lequel il doit être perçu."@fr, "Una categorización que refleja la forma fundamental de comunicación en la cual se expresa el contenido y el sentido humano a través por el se espera sea percibido."@es ;
    rdakit:toolkitLabel "content type"@en, "innehållstyp"@sv, "tipo de contenido"@es, "type de contenu"@fr ;
    reg:hasUnconstrained <http://rdaregistry.info/Elements/u/P60049> ;
    reg:lexicalAlias <http://rdaregistry.info/Elements/e/contentType.en> ;
    reg:name "contentType"@en ;
    reg:status <http://metadataregistry.org/uri/RegStatus/1001> ;
    a rdf:Property ;
    rdfs:domain <http://rdaregistry.info/Elements/c/C10006> ;
    rdfs:isDefinedBy <http://rdaregistry.info/Elements/e/> ;
    rdfs:label "har innehållstyp"@sv, "has content type"@en ;
    skos:definition "Relates an expression to a categorization reflecting the fundamental form of communication in which the content is expressed and the human sense through which it is intended to be perceived."@en ;
    skos:scopeNote "Content type also reflects the number of spatial dimensions and the presence or absence of movement in which content expressed in the form of an image or images is intended to be perceived."@en .

<http://rdaregistry.info/Elements/e/P20002>
    rdakit:instructionNumber "6.13" ;
    rdakit:toolkitDefinition "A character string uniquely associated with an expression, or with a surrogate such as an authority record for an expression."@en, "Chaîne de caractères associée de manière unique à une expression ou à un substitut d’une expression (par exemple, une notice d’autorité), qui sert à distinguer cette expression d’autres expressions."@fr, "Una cadena de caracteres unívocamente asociada con una expresión, o con un substituto de una expresión (p.ej., un registro de autoridad)."@es ;
    rdakit:toolkitLabel "identifiant de l’expression"@fr, "identificador de la expresión"@es, "identifier for expression"@en, "identifikator för uttrycket"@sv ;
    reg:hasUnconstrained <http://rdaregistry.info/Elements/u/P60052> ;
    reg:lexicalAlias <http://rdaregistry.info/Elements/e/identifierForExpression.en> ;
    reg:name "identifierForExpression"@en ;
    reg:status <http://metadataregistry.org/uri/RegStatus/1001> ;
    a rdf:Property ;
    rdfs:domain <http://rdaregistry.info/Elements/c/C10006> ;
    rdfs:isDefinedBy <http://rdaregistry.info/Elements/e/> ;
    rdfs:label "har identifikator för uttrycket"@sv, "has identifier for expression"@en ;
    skos:definition "Relates an expression to a character string uniquely associated with an expression, or with a surrogate such as an authority record for an expression."@en ;
    skos:scopeNote "An identifier serves to differentiate an expression from other expressions."@en .

<http://rdaregistry.info/Elements/e/P20003>
    rdakit:instructionNumber "6.12" ;
    rdakit:toolkitDefinition "A characteristic other than content type, language of expression, or date of expression serving to differentiate an expression from another expression of the same work."@en, "Caractéristique autre que le type de contenu, la langue de l’expression ou la date de l’expression."@fr, "Una característica diferente del tipo de contenido, lengua de expresión o fecha de expresión."@es ;
    rdakit:toolkitLabel "andra särskiljande egenskaper för uttrycket"@sv, "autre caractéristique distinctive de l’expression"@fr, "other distinguishing characteristic of expression"@en, "otra característica distintiva de la expresión"@es ;
    reg:hasUnconstrained <http://rdaregistry.info/Elements/u/P60054> ;
    reg:lexicalAlias <http://rdaregistry.info/Elements/e/otherDistinguishingCharacteristicOfExpression.en> ;
    reg:name "otherDistinguishingCharacteristicOfExpression"@en ;
    reg:status <http://metadataregistry.org/uri/RegStatus/1001> ;
    a rdf:Property ;
    rdfs:domain <http://rdaregistry.info/Elements/c/C10006> ;
    rdfs:isDefinedBy <http://rdaregistry.info/Elements/e/> ;
    rdfs:label "har andra särskiljande egenskaper för uttrycket"@sv, "has other distinguishing characteristic of expression"@en ;
    skos:definition "Relates an expression to a characteristic other than content type, language of expression, or date of expression serving to differentiate an expression from another expression of the same work."@en ;
    skos:scopeNote "Elle sert à distinguer une expression d’une autre expression de la même œuvre."@fr .

<http://rdaregistry.info/Elements/e/P20004>
    rdakit:instructionNumber "7.11.3" ;
    rdakit:toolkitDefinition "A date associated with the recording, filming, etc., of the content of an expression."@en, "La date ou la fourchette de dates associée à la captation (c’est-à-dire l’enregistrement, le tournage, etc.) du contenu de la ressource."@fr, "Una fecha o rango de fechas asociadas con la captura (i.e, grabación, filmación, etc.) del contenido del recurso."@es ;
    rdakit:toolkitLabel "date de captation"@fr, "date of capture"@en, "fecha de captura"@es, "inspelningstid"@sv ;
    reg:hasUnconstrained <http://rdaregistry.info/Elements/u/P60074> ;
    reg:lexicalAlias <http://rdaregistry.info/Elements/e/dateOfCapture.en> ;
    reg:name "dateOfCapture"@en ;
    reg:status <http://metadataregistry.org/uri/RegStatus/1001> ;
    a rdf:Property ;
    rdfs:domain <http://rdaregistry.info/Elements/c/C10006> ;
    rdfs:isDefinedBy <http://rdaregistry.info/Elements/e/> ;
    rdfs:label "har inspelningstid"@sv, "has date of capture"@en ;
    skos:definition "Relates an expression to a date associated with the recording, filming, etc., of the content of an expression."@en .

<http://rdaregistry.info/Elements/e/P20005>
    rdakit:instructionNumber "7.28" ;
    rdakit:toolkitDefinition "A formal recognition of excellence, etc., given by an award- or prize-granting body, for the content of an expression."@en, "Reconnaissance officielle d’excellence, etc. accordée au contenu d’une ressource par un organisme octroyant une récompense ou un prix."@fr, "Un reconocimiento formal de excelencia, etc., otorgado por una entidad que concede premios o reconocimientos, por el contenido de un recurso."@es ;
    rdakit:toolkitLabel "award"@en, "premio"@es, "prix"@fr, "utmärkelse"@sv ;
    reg:hasUnconstrained <http://rdaregistry.info/Elements/u/P60090> ;
    reg:lexicalAlias <http://rdaregistry.info/Elements/e/award.en> ;
    reg:name "award"@en ;
    reg:status <http://metadataregistry.org/uri/RegStatus/1001> ;
    a rdf:Property ;
    rdfs:domain <http://rdaregistry.info/Elements/c/C10006> ;
    rdfs:isDefinedBy <http://rdaregistry.info/Elements/e/> ;
    rdfs:label "har utmärkelse"@sv, "has award"@en ;
    skos:definition "Relates an expression to a formal recognition of excellence, etc., given by an award- or prize-granting body, for the content of an expression."@en .

<http://rdaregistry.info/Elements/e/P20006>
    rdakit:instructionNumber "6.11" ;
    rdakit:toolkitDefinition "A language in which a work is expressed."@en, "Langue dans laquelle une œuvre est exprimée."@fr, "Una lengua en la que se expresa una obra"@es ;
    rdakit:toolkitLabel "language of expression"@en, "langue de l’expression"@fr, "lengua de la expresión"@es ;
    reg:hasUnconstrained <http://rdaregistry.info/Elements/u/P60099> ;
    reg:lexicalAlias <http://rdaregistry.info/Elements/e/languageOfExpression.en> ;
    reg:name "languageOfExpression"@en ;
    reg:status <http://metadataregistry.org/uri/RegStatus/1001> ;
    a rdf:Property ;
    rdfs:domain <http://rdaregistry.info/Elements/c/C10006> ;
    rdfs:isDefinedBy <http://rdaregistry.info/Elements/e/> ;
    rdfs:label "has language of expression"@en ;
    skos:definition "Relates an expression to a language in which a work is expressed."@en .

<http://rdaregistry.info/Elements/e/P20007>
    rdakit:instructionNumber "7.12" ;
    rdakit:toolkitDefinition "A language used to express the content of an expression."@en, "Langue utilisée pour exprimer le contenu d’une ressource."@fr, "Una lengua utilizada para expresar el contenido de un recurso."@es ;
    rdakit:toolkitLabel "language of content"@en, "langue du contenu"@fr, "lengua del contenido"@es ;
    reg:hasUnconstrained <http://rdaregistry.info/Elements/u/P60099> ;
    reg:lexicalAlias <http://rdaregistry.info/Elements/e/languageOfContent.en> ;
    reg:name "languageOfContent"@en ;
    reg:status <http://metadataregistry.org/uri/RegStatus/1001> ;
    a rdf:Property ;
    rdfs:domain <http://rdaregistry.info/Elements/c/C10006> ;
    rdfs:isDefinedBy <http://rdaregistry.info/Elements/e/> ;
    rdfs:label "has language of content"@en ;
    skos:definition "Relates an expression to a language used to express the content of an expression."@en .

<http://rdaregistry.info/Elements/e/P20008>
    reg:status <http://metadataregistry.org/uri/RegStatus/1008> ;
    a rdf:Property ;
    rdfs:isDefinedBy <http://rdaregistry.info/Elements/e/> .

<http://rdaregistry.info/Elements/e/P20009>
    rdakit:instructionNumber "24.5" ;
    rdakit:toolkitDefinition "A motion picture based on a source expression."@en, "Film basé sur l’expression source."@fr, "Una película cinematográfica basada en la expresión fuente."@es ;
    rdakit:toolkitLabel "adaptada como película cinematográfica (expresión)"@es, "adapted as motion picture (expression)"@en, "adapté en film (expression)"@fr ;
    reg:hasSubproperty <http://rdaregistry.info/Elements/e/object/P20009> ;
    reg:hasUnconstrained <http://rdaregistry.info/Elements/u/P60110> ;
    reg:lexicalAlias <http://rdaregistry.info/Elements/e/adaptedAsMotionPictureExpression.en> ;
    reg:name "adaptedAsMotionPictureExpression"@en ;
    reg:status <http://metadataregistry.org/uri/RegStatus/1001> ;
    a rdf:Property ;
    rdfs:domain <http://rdaregistry.info/Elements/c/C10006> ;
    rdfs:isDefinedBy <http://rdaregistry.info/Elements/e/> ;
    rdfs:label "is adapted as motion picture (expression)"@en ;
    rdfs:subPropertyOf <http://rdaregistry.info/Elements/e/P20153> ;
    skos:definition "Relates an expression to a motion picture based on a source expression."@en .

<http://rdaregistry.info/Elements/e/P20010>
    rdakit:instructionNumber "7.29.2" ;
    rdakit:toolkitDefinition "A note on changes in content characteristics that occur in subsequent issues or parts of an expression issued in successive parts or between iterations of an integrating resource."@en, "Note portant sur les changements de caractéristiques du contenu survenant dans les livraisons ou les parties ultérieures d’une ressource publiée en parties successives ou bien entre les différentes itérations d’une ressource intégratrice."@fr, "Una nota sobre cambios en las características que ocurren en entregas o partes subsecuentes de un recurso publicado en partes sucesivas o entre iteraciones de un recurso integrable."@es ;
    rdakit:toolkitLabel "anmärkning om förändringar i innehållsegenskaper"@sv, "nota sobre cambios en las características del contenido"@es, "note on changes in content characteristics"@en, "note relative aux changements de caractéristiques du contenu"@fr ;
    reg:hasUnconstrained <http://rdaregistry.info/Elements/u/P60123> ;
    reg:lexicalAlias <http://rdaregistry.info/Elements/e/noteOnChangesInContentCharacteristics.en> ;
    reg:name "noteOnChangesInContentCharacteristics"@en ;
    reg:status <http://metadataregistry.org/uri/RegStatus/1001> ;
    a rdf:Property ;
    rdfs:domain <http://rdaregistry.info/Elements/c/C10006> ;
    rdfs:isDefinedBy <http://rdaregistry.info/Elements/e/> ;
    rdfs:label "har anmärkning om förändringar i innehållsegenskaper"@sv, "has note on changes in content characteristics"@en ;
    rdfs:subPropertyOf <http://rdaregistry.info/Elements/e/P20071> ;
    skos:definition "Relates an expression to a note on changes in content characteristics that occur in subsequent issues or parts of an expression issued in successive parts or between iterations of an integrating resource."@en .

<http://rdaregistry.info/Elements/e/P20011>
    rdakit:instructionNumber "18.5" ;
    rdakit:toolkitDefinition "A performer contributing to an expression of a musical work by leading a performing group in a musical or dramatic presentation, etc."@en, "Interprète contribuant à une expression d’une œuvre musicale en dirigeant un groupe d’interprètes (orchestre, chorale, opéra, etc.) dans une représentation musicale ou dramatique, etc."@fr, "Un intérprete que contribuye a una expresión de una obra musical dirigiendo un grupo de interpretación (orquesta, coro, ópera, etc.) en una presentación musical o teatral, etc."@es ;
    rdakit:toolkitLabel "chef d’orchestre"@fr, "conductor"@en, "director de orquesta"@es ;
    reg:hasSubproperty <http://rdaregistry.info/Elements/e/P20285>, <http://rdaregistry.info/Elements/e/P20286>, <http://rdaregistry.info/Elements/e/object/P20011> ;
    reg:hasUnconstrained <http://rdaregistry.info/Elements/u/P60141> ;
    reg:lexicalAlias <http://rdaregistry.info/Elements/e/conductor.en> ;
    reg:name "conductor"@en ;
    reg:status <http://metadataregistry.org/uri/RegStatus/1001> ;
    a rdf:Property ;
    rdfs:domain <http://rdaregistry.info/Elements/c/C10006> ;
    rdfs:isDefinedBy <http://rdaregistry.info/Elements/e/> ;
    rdfs:label "has conductor"@en ;
    rdfs:subPropertyOf <http://rdaregistry.info/Elements/e/P20039> ;
    skos:definition "Relates an expression to a performer contributing to an expression of a musical work by leading a performing group in a musical or dramatic presentation, etc."@en .

<http://rdaregistry.info/Elements/e/P20012>
    rdakit:instructionNumber "18.5" ;
    rdakit:toolkitDefinition "A performer contributing to an expression of a work by acting as a cast member or player in a musical or dramatic presentation, etc."@en, "Interprète contribuant à une expression d’une œuvre en agissant à titre de membre d’une distribution artistique ou de comédien dans une représentation musicale ou dramatique, etc."@fr, "Un intérprete que contribuye a una expresión de una obra actuando como un miembro de un reparto o actor en una producción musical o teatral, etc."@es ;
    rdakit:toolkitLabel "acteur"@fr, "actor"@en, "actor"@es ;
    reg:hasSubproperty <http://rdaregistry.info/Elements/e/P20070>, <http://rdaregistry.info/Elements/e/object/P20012> ;
    reg:hasUnconstrained <http://rdaregistry.info/Elements/u/P60142> ;
    reg:lexicalAlias <http://rdaregistry.info/Elements/e/actor.en> ;
    reg:name "actor"@en ;
    reg:status <http://metadataregistry.org/uri/RegStatus/1001> ;
    a rdf:Property ;
    rdfs:domain <http://rdaregistry.info/Elements/c/C10006> ;
    rdfs:isDefinedBy <http://rdaregistry.info/Elements/e/> ;
    rdfs:label "has actor"@en ;
    rdfs:subPropertyOf <http://rdaregistry.info/Elements/e/P20039> ;
    skos:definition "Relates an expression to a performer contributing to an expression of a work by acting as a cast member or player in a musical or dramatic presentation, etc."@en .

<http://rdaregistry.info/Elements/e/P20013>
    rdakit:instructionNumber "18.5" ;
    rdakit:seeAlso <http://rdaregistry.info/Elements/e/P20279> ;
    rdakit:toolkitDefinition "A performer contributing to an expression of a work by appearing on screen to provide contextual or background information."@en, "Interprète contribuant à une expression d’une œuvre en apparaissant à l’écran pour fournir de l’information contextuelle ou complémentaire."@fr, "Un intérprete que contribuye a una expresión de una obra para ofrecer en pantalla información contextual o básica."@es ;
    rdakit:toolkitLabel "on-screen presenter"@en, "presentador en pantalla"@es, "présentateur à l’écran"@fr ;
    reg:hasSubproperty <http://rdaregistry.info/Elements/e/object/P20013> ;
    reg:hasUnconstrained <http://rdaregistry.info/Elements/u/P60143> ;
    reg:lexicalAlias <http://rdaregistry.info/Elements/e/onScreenPresenter.en> ;
    reg:name "onScreenPresenter"@en ;
    reg:status <http://metadataregistry.org/uri/RegStatus/1001> ;
    a rdf:Property ;
    rdfs:domain <http://rdaregistry.info/Elements/c/C10006> ;
    rdfs:isDefinedBy <http://rdaregistry.info/Elements/e/> ;
    rdfs:label "has on-screen presenter"@en ;
    rdfs:subPropertyOf <http://rdaregistry.info/Elements/e/P20039> ;
    skos:definition "Relates an expression to a performer contributing to an expression of a work by appearing on screen to provide contextual or background information."@en ;
    skos:scopeNote "Appearance in nonfiction moving image materials or in introductions to fiction moving image materials is included. Appearance on screen in a non-performing role is excluded."@en .

<http://rdaregistry.info/Elements/e/P20014>
    rdakit:instructionNumber "18.5" ;
    rdakit:toolkitDefinition "A performer contributing to an expression of a work by dancing in a musical, dramatic, etc., presentation."@en, "Interprète contribuant à une expression d’une œuvre en dansant dans une représentation musicale ou dramatique, etc."@fr, "Un intérprete que contribuye a una expresión de una obra danzando en una presentación musical, dramática, etc."@es ;
    rdakit:toolkitLabel "bailarín"@es, "dancer"@en, "danseur"@fr ;
    reg:hasSubproperty <http://rdaregistry.info/Elements/e/object/P20014> ;
    reg:hasUnconstrained <http://rdaregistry.info/Elements/u/P60144> ;
    reg:lexicalAlias <http://rdaregistry.info/Elements/e/dancer.en> ;
    reg:name "dancer"@en ;
    reg:status <http://metadataregistry.org/uri/RegStatus/1001> ;
    a rdf:Property ;
    rdfs:domain <http://rdaregistry.info/Elements/c/C10006> ;
    rdfs:isDefinedBy <http://rdaregistry.info/Elements/e/> ;
    rdfs:label "has dancer"@en ;
    rdfs:subPropertyOf <http://rdaregistry.info/Elements/e/P20039> ;
    skos:definition "Relates an expression to a performer contributing to an expression of a work by dancing in a musical, dramatic, etc., presentation."@en .

<http://rdaregistry.info/Elements/e/P20015>
    rdakit:instructionNumber "18.5" ;
    rdakit:toolkitDefinition "A performer contributing to an expression of a work by teaching or providing a demonstration."@en, "Interprète contribuant à une expression d’une œuvre en transmettant des connaissances par la théorie ou la pratique."@fr, "Un intérprete que contribuye a una expresión de una obra impartiendo formación o proporcionando una demostración."@es ;
    rdakit:toolkitLabel "enseignant"@fr, "instructor"@en, "profesor"@es ;
    reg:hasSubproperty <http://rdaregistry.info/Elements/e/object/P20015> ;
    reg:hasUnconstrained <http://rdaregistry.info/Elements/u/P60145> ;
    reg:lexicalAlias <http://rdaregistry.info/Elements/e/instructor.en> ;
    reg:name "instructor"@en ;
    reg:status <http://metadataregistry.org/uri/RegStatus/1001> ;
    a rdf:Property ;
    rdfs:domain <http://rdaregistry.info/Elements/c/C10006> ;
    rdfs:isDefinedBy <http://rdaregistry.info/Elements/e/> ;
    rdfs:label "has instructor"@en ;
    rdfs:subPropertyOf <http://rdaregistry.info/Elements/e/P20039> ;
    skos:definition "Relates an expression to a performer contributing to an expression of a work by teaching or providing a demonstration."@en .

<http://rdaregistry.info/Elements/e/P20016>
    rdakit:instructionNumber "18.5" ;
    rdakit:toolkitDefinition "A performer contributing to an expression of a work by leading a program, often broadcast, that includes other guests, performers, etc."@en, "Interprète contribuant à une expression d’une œuvre en dirigeant une émission (souvent diffusée) qui comprend d’autres invités, interprètes, etc. (par exemple, un animateur d’émission-débat)."@fr, "Un intérprete que contribuye a una expresión de una obra dirigiendo un programa (a menudo una transmisión) que incluye otros invitados, intérpretes, etc., ( por ej., presentadores de programas de debates)."@es ;
    rdakit:toolkitLabel "host"@en, "hôte"@fr, "presentador"@es ;
    reg:hasSubproperty <http://rdaregistry.info/Elements/e/object/P20016> ;
    reg:hasUnconstrained <http://rdaregistry.info/Elements/u/P60146> ;
    reg:lexicalAlias <http://rdaregistry.info/Elements/e/host.en> ;
    reg:name "host"@en ;
    reg:status <http://metadataregistry.org/uri/RegStatus/1001> ;
    a rdf:Property ;
    rdfs:domain <http://rdaregistry.info/Elements/c/C10006> ;
    rdfs:isDefinedBy <http://rdaregistry.info/Elements/e/> ;
    rdfs:label "has host"@en ;
    rdfs:subPropertyOf <http://rdaregistry.info/Elements/e/P20039> ;
    skos:definition "Relates an expression to a performer contributing to an expression of a work by leading a program, often broadcast, that includes other guests, performers, etc."@en .

<http://rdaregistry.info/Elements/e/P20017>
    rdakit:instructionNumber "18.5" ;
    rdakit:toolkitDefinition "A performer contributing to an expression of a work by leading a program, often broadcast, where topics are discussed, usually with participation of experts in fields related to the discussion."@en, "Interprète contribuant à une expression d’une œuvre en dirigeant une émission (souvent diffusée) où des sujets sont discutés, habituellement avec la participation d’experts dans les domaines reliés à la discussion."@fr, "Un intérprete que contribuye a una expresión de una obra dirigiendo un programa (a menudo una transmisión) en el cual los temas se discuten generalmente con la participación de expertos en esos temas."@es ;
    rdakit:toolkitLabel "moderador"@es, "moderator"@en, "modérateur"@fr ;
    reg:hasSubproperty <http://rdaregistry.info/Elements/e/object/P20017> ;
    reg:hasUnconstrained <http://rdaregistry.info/Elements/u/P60147> ;
    reg:lexicalAlias <http://rdaregistry.info/Elements/e/moderator.en> ;
    reg:name "moderator"@en ;
    reg:status <http://metadataregistry.org/uri/RegStatus/1001> ;
    a rdf:Property ;
    rdfs:domain <http://rdaregistry.info/Elements/c/C10006> ;
    rdfs:isDefinedBy <http://rdaregistry.info/Elements/e/> ;
    rdfs:label "has moderator"@en ;
    rdfs:subPropertyOf <http://rdaregistry.info/Elements/e/P20039> ;
    skos:definition "Relates an expression to a performer contributing to an expression of a work by leading a program, often broadcast, where topics are discussed, usually with participation of experts in fields related to the discussion."@en .

<http://rdaregistry.info/Elements/e/P20018>
    rdakit:instructionNumber "18.5" ;
    rdakit:toolkitDefinition "A performer contributing to an expression of a work by manipulating, controlling, or directing puppets or marionettes in a moving image production or a musical or dramatic presentation or entertainment."@en, "Interprète contribuant à une expression d’une œuvre en manipulant, en contrôlant ou en dirigeant des marionnettes dans une production d’images animées ou bien dans une représentation ou un spectacle musical ou dramatique."@fr, "Un intérprete que contribuye a una expresión de una obra manipulando, controlando o dirigiendo títeres o marionetas en una producción de imágenes en movimiento o producción teatral, musical o un espectáculo."@es ;
    rdakit:toolkitLabel "marionnettiste"@fr, "puppeteer"@en, "titiritero"@es ;
    reg:hasSubproperty <http://rdaregistry.info/Elements/e/object/P20018> ;
    reg:hasUnconstrained <http://rdaregistry.info/Elements/u/P60148> ;
    reg:lexicalAlias <http://rdaregistry.info/Elements/e/puppeteer.en> ;
    reg:name "puppeteer"@en ;
    reg:status <http://metadataregistry.org/uri/RegStatus/1001> ;
    a rdf:Property ;
    rdfs:domain <http://rdaregistry.info/Elements/c/C10006> ;
    rdfs:isDefinedBy <http://rdaregistry.info/Elements/e/> ;
    rdfs:label "has puppeteer"@en ;
    rdfs:subPropertyOf <http://rdaregistry.info/Elements/e/P20039> ;
    skos:definition "Relates an expression to a performer contributing to an expression of a work by manipulating, controlling, or directing puppets or marionettes in a moving image production or a musical or dramatic presentation or entertainment."@en .

<http://rdaregistry.info/Elements/e/P20019>
    rdakit:instructionNumber "18.5" ;
    rdakit:toolkitDefinition "A performer contributing to an expression of a work by participating in a program, often broadcast, where topics are discussed, usually with participation of experts in fields related to the discussion."@en, "Interprète contribuant à une expression d’une œuvre en participant à une émission (souvent diffusée) où des sujets sont discutés, habituellement avec la participation d’experts dans les domaines reliés à la discussion."@fr, "Un intérprete que contribuye a una expresión de una obra participando en un programa (a menudo una transmisión) en el cual los temas se discuten generalmente con la participación de expertos en esos temas."@es ;
    rdakit:toolkitLabel "panelist"@en, "panelista"@es, "panéliste"@fr ;
    reg:hasSubproperty <http://rdaregistry.info/Elements/e/object/P20019> ;
    reg:hasUnconstrained <http://rdaregistry.info/Elements/u/P60149> ;
    reg:lexicalAlias <http://rdaregistry.info/Elements/e/panelist.en> ;
    reg:name "panelist"@en ;
    reg:status <http://metadataregistry.org/uri/RegStatus/1001> ;
    a rdf:Property ;
    rdfs:domain <http://rdaregistry.info/Elements/c/C10006> ;
    rdfs:isDefinedBy <http://rdaregistry.info/Elements/e/> ;
    rdfs:label "has panelist"@en ;
    rdfs:subPropertyOf <http://rdaregistry.info/Elements/e/P20039> ;
    skos:definition "Relates an expression to a performer contributing to an expression of a work by participating in a program, often broadcast, where topics are discussed, usually with participation of experts in fields related to the discussion."@en .

<http://rdaregistry.info/Elements/e/P20020>
    rdakit:instructionNumber "18.5" ;
    rdakit:toolkitDefinition "A performer contributing to an expression of a work by playing a musical instrument."@en, "Interprète contribuant à une expression d’une œuvre en jouant d’un instrument de musique."@fr, "Un intérprete que contribuye a una expresión de una obra tocando un instrumento musical."@es ;
    rdakit:toolkitLabel "instrumentalist"@en, "instrumentista"@es, "instrumentiste"@fr ;
    reg:hasSubproperty <http://rdaregistry.info/Elements/e/object/P20020> ;
    reg:hasUnconstrained <http://rdaregistry.info/Elements/u/P60150> ;
    reg:lexicalAlias <http://rdaregistry.info/Elements/e/instrumentalist.en> ;
    reg:name "instrumentalist"@en ;
    reg:status <http://metadataregistry.org/uri/RegStatus/1001> ;
    a rdf:Property ;
    rdfs:domain <http://rdaregistry.info/Elements/c/C10006> ;
    rdfs:isDefinedBy <http://rdaregistry.info/Elements/e/> ;
    rdfs:label "has instrumentalist"@en ;
    rdfs:subPropertyOf <http://rdaregistry.info/Elements/e/P20039> ;
    skos:definition "Relates an expression to a performer contributing to an expression of a work by playing a musical instrument."@en .

<http://rdaregistry.info/Elements/e/P20021>
    rdakit:instructionNumber "18.5" ;
    rdakit:toolkitDefinition "A performer contributing to an expression of a work by providing interpretation, analysis, or a discussion of the subject matter on a recording, film, or other audiovisual medium."@en, "Interprète contribuant à une expression d’une œuvre en fournissant une interprétation, une analyse ou une explication du sujet sur un enregistrement, un film ou un autre support audiovisuel."@fr, "Un intérprete que contribuye a una expresión de una obra dando una interpretación, análisis, o una discusión del tema en una grabación, película u otro medio audiovisual."@es ;
    rdakit:toolkitLabel "comentarista"@es, "commentateur"@fr, "commentator"@en ;
    reg:hasSubproperty <http://rdaregistry.info/Elements/e/object/P20021> ;
    reg:hasUnconstrained <http://rdaregistry.info/Elements/u/P60151> ;
    reg:lexicalAlias <http://rdaregistry.info/Elements/e/commentator.en> ;
    reg:name "commentator"@en ;
    reg:status <http://metadataregistry.org/uri/RegStatus/1001> ;
    a rdf:Property ;
    rdfs:domain <http://rdaregistry.info/Elements/c/C10006> ;
    rdfs:isDefinedBy <http://rdaregistry.info/Elements/e/> ;
    rdfs:label "has commentator"@en ;
    rdfs:subPropertyOf <http://rdaregistry.info/Elements/e/P20039> ;
    skos:definition "Relates an expression to a performer contributing to an expression of a work by providing interpretation, analysis, or a discussion of the subject matter on a recording, film, or other audiovisual medium."@en .

<http://rdaregistry.info/Elements/e/P20022>
    rdakit:instructionNumber "18.5" ;
    rdakit:toolkitDefinition "A performer contributing to an expression of a work by reading aloud or giving an account of an act, occurrence, course of events, etc."@en, "Interprète contribuant à une expression d’une œuvre en lisant à voix haute ou en rendant compte d’une action, d’une situation, du déroulement des événements, etc."@fr, "Un intérprete que contribuye a una expresión de una obra leyendo en voz alta o hablando para dar cuenta de un acto, acontecimiento, desarrollo de eventos, etc."@es ;
    rdakit:toolkitLabel "narrador"@es, "narrateur"@fr, "narrator"@en ;
    reg:hasSubproperty <http://rdaregistry.info/Elements/e/object/P20022> ;
    reg:hasUnconstrained <http://rdaregistry.info/Elements/u/P60153> ;
    reg:lexicalAlias <http://rdaregistry.info/Elements/e/narrator.en> ;
    reg:name "narrator"@en ;
    reg:status <http://metadataregistry.org/uri/RegStatus/1001> ;
    a rdf:Property ;
    rdfs:domain <http://rdaregistry.info/Elements/c/C10006> ;
    rdfs:isDefinedBy <http://rdaregistry.info/Elements/e/> ;
    rdfs:label "has narrator"@en ;
    rdfs:subPropertyOf <http://rdaregistry.info/Elements/e/P20039> ;
    skos:definition "Relates an expression to a performer contributing to an expression of a work by reading aloud or giving an account of an act, occurrence, course of events, etc."@en .

<http://rdaregistry.info/Elements/e/P20023>
    rdakit:instructionNumber "18.5" ;
    rdakit:toolkitDefinition "A performer contributing to an expression of a work by relaying a creator's original story with dramatic or theatrical interpretation."@en, "Interprète contribuant à une expression d’une œuvre en racontant l’histoire originale d’un créateur dans une interprétation dramatique ou théâtrale."@fr, "Un intérprete que contribuye a una expresión de una obra contando una historia de un creador original mediante una interpretación dramática o teatral."@es ;
    rdakit:toolkitLabel "conteur"@fr, "narrador de cuentos"@es, "storyteller"@en ;
    reg:hasSubproperty <http://rdaregistry.info/Elements/e/object/P20023> ;
    reg:hasUnconstrained <http://rdaregistry.info/Elements/u/P60154> ;
    reg:lexicalAlias <http://rdaregistry.info/Elements/e/storyteller.en> ;
    reg:name "storyteller"@en ;
    reg:status <http://metadataregistry.org/uri/RegStatus/1001> ;
    a rdf:Property ;
    rdfs:domain <http://rdaregistry.info/Elements/c/C10006> ;
    rdfs:isDefinedBy <http://rdaregistry.info/Elements/e/> ;
    rdfs:label "has storyteller"@en ;
    rdfs:subPropertyOf <http://rdaregistry.info/Elements/e/P20039> ;
    skos:definition "Relates an expression to a performer contributing to an expression of a work by relaying a creator's original story with dramatic or theatrical interpretation."@en .

<http://rdaregistry.info/Elements/e/P20024>
    rdakit:instructionNumber "18.5" ;
    rdakit:toolkitDefinition "A performer contributing to an expression of a work by speaking words, such as a lecture, speech, etc."@en, "Interprète contribuant à une expression d’une œuvre en énonçant des paroles, telles qu’un exposé, un discours, etc."@fr, "Un intérprete que contribuye a una expresión de una obra haciendo u ofreciendo conferencias, discursos, etc."@es ;
    rdakit:toolkitLabel "conferenciante"@es, "orateur"@fr, "speaker"@en ;
    reg:hasSubproperty <http://rdaregistry.info/Elements/e/object/P20024> ;
    reg:hasUnconstrained <http://rdaregistry.info/Elements/u/P60155> ;
    reg:lexicalAlias <http://rdaregistry.info/Elements/e/speaker.en> ;
    reg:name "speaker"@en ;
    reg:status <http://metadataregistry.org/uri/RegStatus/1001> ;
    a rdf:Property ;
    rdfs:domain <http://rdaregistry.info/Elements/c/C10006> ;
    rdfs:isDefinedBy <http://rdaregistry.info/Elements/e/> ;
    rdfs:label "has speaker"@en ;
    rdfs:subPropertyOf <http://rdaregistry.info/Elements/e/P20039> ;
    skos:definition "Relates an expression to a performer contributing to an expression of a work by speaking words, such as a lecture, speech, etc."@en .

<http://rdaregistry.info/Elements/e/P20025>
    rdakit:instructionNumber "18.5" ;
    rdakit:toolkitDefinition "A performer contributing to an expression of a work by using his/her/their voice, with or without instrumental accompaniment, to produce music."@en, "Interprète contribuant à une expression d’une œuvre en utilisant sa voix, avec ou sans accompagnement instrumental, pour produire de la musique."@fr, "Un intérprete que contribuye a una expresión de una obra usando su voz, sus voces, con o sin acompañamiento instrumental, para producir música."@es ;
    rdakit:toolkitLabel "cantante"@es, "chanteur"@fr, "singer"@en ;
    reg:hasSubproperty <http://rdaregistry.info/Elements/e/object/P20025> ;
    reg:hasUnconstrained <http://rdaregistry.info/Elements/u/P60156> ;
    reg:lexicalAlias <http://rdaregistry.info/Elements/e/singer.en> ;
    reg:name "singer"@en ;
    reg:status <http://metadataregistry.org/uri/RegStatus/1001> ;
    a rdf:Property ;
    rdfs:domain <http://rdaregistry.info/Elements/c/C10006> ;
    rdfs:isDefinedBy <http://rdaregistry.info/Elements/e/> ;
    rdfs:label "has singer"@en ;
    rdfs:subPropertyOf <http://rdaregistry.info/Elements/e/P20039> ;
    skos:definition "Relates an expression to a performer contributing to an expression of a work by using his/her/their voice, with or without instrumental accompaniment, to produce music."@en ;
    skos:scopeNote "A singer's performance may or may not include actual words."@en .

<http://rdaregistry.info/Elements/e/P20026>
    rdakit:instructionNumber "18.5" ;
    rdakit:toolkitDefinition "An agent contributing to an expression by adding music to a work that originally lacked it, by composing new music to substitute for original music, or by composing new music to supplement existing music."@en, "Personne, famille ou collectivité contribuant à une expression en ajoutant de la musique à une œuvre qui n’en avait pas à l’origine, en composant une nouvelle musique pour remplacer la musique originale ou en composant une nouvelle musique pour compléter la musique existante."@fr, "Una persona, familia o entidad corporativa que contribuye a una expresión agregando música a una obra que originalmente no tenía, componiendo música nueva para sustituir la música original, o componiendo nueva música para complementar la música existente."@es ;
    rdakit:toolkitLabel "composer (expression)"@en, "compositeur (expression)"@fr, "compositor (expresión)"@es ;
    reg:hasSubproperty <http://rdaregistry.info/Elements/e/object/P20026> ;
    reg:hasUnconstrained <http://rdaregistry.info/Elements/u/P60426> ;
    reg:lexicalAlias <http://rdaregistry.info/Elements/e/composerExpression.en> ;
    reg:name "composerExpression"@en ;
    reg:status <http://metadataregistry.org/uri/RegStatus/1001> ;
    a rdf:Property ;
    rdfs:domain <http://rdaregistry.info/Elements/c/C10006> ;
    rdfs:isDefinedBy <http://rdaregistry.info/Elements/e/> ;
    rdfs:label "has composer (expression)"@en ;
    rdfs:subPropertyOf <http://rdaregistry.info/Elements/e/P20053> ;
    skos:definition "Relates an expression to an agent contributing to an expression by adding music to a work that originally lacked it, by composing new music to substitute for original music, or by composing new music to supplement existing music."@en .

<http://rdaregistry.info/Elements/e/P20027>
    rdakit:instructionNumber "18.5" ;
    rdakit:toolkitDefinition "An agent contributing to an expression of a cartographic work by providing measurements or dimensional relationships for a geographic area represented."@en, "Personne, famille ou collectivité contribuant à une expression d’une œuvre cartographique en fournissant les mesures ou les relations dimensionnelles pour  l’aire géographique représentée."@fr, "Una persona, familia o entidad corporativa que contribuye a una expresión de una obra cartográfica proporcionando medidas o relaciones dimensionales para el área geográfica representada."@es ;
    rdakit:toolkitLabel "arpenteur"@fr, "surveyor"@en, "topógrafo"@es ;
    reg:hasSubproperty <http://rdaregistry.info/Elements/e/object/P20027> ;
    reg:hasUnconstrained <http://rdaregistry.info/Elements/u/P60377> ;
    reg:lexicalAlias <http://rdaregistry.info/Elements/e/surveyor.en> ;
    reg:name "surveyor"@en ;
    reg:status <http://metadataregistry.org/uri/RegStatus/1001> ;
    a rdf:Property ;
    rdfs:domain <http://rdaregistry.info/Elements/c/C10006> ;
    rdfs:isDefinedBy <http://rdaregistry.info/Elements/e/> ;
    rdfs:label "has surveyor"@en ;
    rdfs:subPropertyOf <http://rdaregistry.info/Elements/e/P20053> ;
    skos:definition "Relates an expression to an agent contributing to an expression of a cartographic work by providing measurements or dimensional relationships for a geographic area represented."@en .

<http://rdaregistry.info/Elements/e/P20028>
    rdakit:instructionNumber "18.5" ;
    rdakit:seeAlso <http://rdaregistry.info/Elements/w/P10058> ;
    rdakit:toolkitDefinition "An agent contributing to an expression of a moving image work or computer program by giving apparent movement to inanimate objects or drawings."@en, "Personne, famille ou collectivité contribuant à une expression d’une œuvre d’images animées ou d’un programme informatique en donnant l’illusion du mouvement à des objets inanimés ou à des dessins."@fr, "Una persona, familia o entidad corporativa que contribuye a una expresión de una obra de imagen en movimiento o un programa de computadora dando movimiento aparente a objetos o dibujos inanimados."@es ;
    rdakit:toolkitLabel "animador"@es, "animateur"@fr, "animator"@en ;
    reg:hasSubproperty <http://rdaregistry.info/Elements/e/object/P20028> ;
    reg:hasUnconstrained <http://rdaregistry.info/Elements/u/P60378> ;
    reg:lexicalAlias <http://rdaregistry.info/Elements/e/animator.en> ;
    reg:name "animator"@en ;
    reg:status <http://metadataregistry.org/uri/RegStatus/1001> ;
    a rdf:Property ;
    rdfs:domain <http://rdaregistry.info/Elements/c/C10006> ;
    rdfs:isDefinedBy <http://rdaregistry.info/Elements/e/> ;
    rdfs:label "has animator"@en ;
    rdfs:subPropertyOf <http://rdaregistry.info/Elements/e/P20053> ;
    skos:definition "Relates an expression to an agent contributing to an expression of a moving image work or computer program by giving apparent movement to inanimate objects or drawings."@en ;
    skos:scopeNote "Creation of the drawings that are animated is excluded."@en .

<http://rdaregistry.info/Elements/e/P20029>
    rdakit:instructionNumber "18.5" ;
    rdakit:seeAlso <http://rdaregistry.info/Elements/w/P10053> ;
    rdakit:toolkitDefinition "An agent contributing to an expression of a musical work by rewriting a composition for a medium of performance different from that for which a work was originally intended."@en, "Personne, famille ou collectivité contribuant à une expression d’une œuvre musicale en réécrivant la composition pour une distribution d’exécution différente de celle à laquelle l’œuvre est originellement destinée."@fr, "Una persona, familia o entidad corporativa que contribuye a una expresión de una obra musical reescribiendo la composición para un medio de una interpretación diferente de aquel para el que se habia concebido la obra."@es ;
    rdakit:toolkitLabel "arranger of music"@en, "arrangeur de musique"@fr, "arreglista musical"@es ;
    reg:hasSubproperty <http://rdaregistry.info/Elements/e/object/P20029> ;
    reg:hasUnconstrained <http://rdaregistry.info/Elements/u/P60379> ;
    reg:lexicalAlias <http://rdaregistry.info/Elements/e/arrangerOfMusic.en> ;
    reg:name "arrangerOfMusic"@en ;
    reg:status <http://metadataregistry.org/uri/RegStatus/1001> ;
    a rdf:Property ;
    rdfs:domain <http://rdaregistry.info/Elements/c/C10006> ;
    rdfs:isDefinedBy <http://rdaregistry.info/Elements/e/> ;
    rdfs:label "has arranger of music"@en ;
    rdfs:subPropertyOf <http://rdaregistry.info/Elements/e/P20053> ;
    skos:definition "Relates an expression to an agent contributing to an expression of a musical work by rewriting a composition for a medium of performance different from that for which a work was originally intended."@en ;
    skos:scopeNote "Contribution includes modification of a work for the same medium of performance, etc., keeping the musical substance of the original composition essentially unchanged, and excludes substantial modification that results in the creation of a new musical work."@en .

<http://rdaregistry.info/Elements/e/P20030>
    rdakit:instructionNumber "18.5" ;
    rdakit:toolkitDefinition "An agent contributing to an expression of a primarily non-textual work by providing text, such as writing captions for photographs or descriptions of maps."@en, "Personne, famille ou collectivité contribuant à une expression d’une œuvre essentiellement non textuelle en fournissant un texte pour l’œuvre non textuelle (par exemple, en écrivant des légendes pour des photographies, des descriptions de cartes géographiques)."@fr, "Una persona, familia o entidad corporativa que contribuye a una expresión de una obra que no es básicamente texto ofreciendo texto para la obra no textual (por ej., titulación de fotografías, descripción de mapas)."@es ;
    rdakit:toolkitLabel "auteur de texte ajouté"@fr, "autor de texto adicional"@es, "writer of added text"@en ;
    reg:hasSubproperty <http://rdaregistry.info/Elements/e/P20068>, <http://rdaregistry.info/Elements/e/object/P20030> ;
    reg:hasUnconstrained <http://rdaregistry.info/Elements/u/P60380> ;
    reg:lexicalAlias <http://rdaregistry.info/Elements/e/writerOfAddedText.en> ;
    reg:name "writerOfAddedText"@en ;
    reg:status <http://metadataregistry.org/uri/RegStatus/1001> ;
    a rdf:Property ;
    rdfs:domain <http://rdaregistry.info/Elements/c/C10006> ;
    rdfs:isDefinedBy <http://rdaregistry.info/Elements/e/> ;
    rdfs:label "has writer of added text"@en ;
    rdfs:subPropertyOf <http://rdaregistry.info/Elements/e/P20046> ;
    skos:definition "Relates an expression to an agent contributing to an expression of a primarily non-textual work by providing text, such as writing captions for photographs or descriptions of maps."@en .

<http://rdaregistry.info/Elements/e/P20031>
    rdakit:instructionNumber "18.5" ;
    rdakit:toolkitDefinition "An agent contributing to an expression of a stage work through the general management and supervision of a performance."@en, "Personne, famille ou collectivité contribuant à une expression d’une œuvre scénique par la gestion et la supervision générales d’une prestation."@fr, "Una persona, familia o entidad corporativa que contribuye a una expresión de una obra escénica mediante la dirección y supervisión general de una interpretación."@es ;
    rdakit:toolkitLabel "director de escena"@es, "metteur en scène"@fr, "stage director"@en ;
    reg:hasSubproperty <http://rdaregistry.info/Elements/e/object/P20031> ;
    reg:hasUnconstrained <http://rdaregistry.info/Elements/u/P60399> ;
    reg:lexicalAlias <http://rdaregistry.info/Elements/e/stageDirector.en> ;
    reg:name "stageDirector"@en ;
    reg:status <http://metadataregistry.org/uri/RegStatus/1001> ;
    a rdf:Property ;
    rdfs:domain <http://rdaregistry.info/Elements/c/C10006> ;
    rdfs:isDefinedBy <http://rdaregistry.info/Elements/e/> ;
    rdfs:label "has stage director"@en ;
    rdfs:subPropertyOf <http://rdaregistry.info/Elements/e/P20053> ;
    skos:definition "Relates an expression to an agent contributing to an expression of a stage work through the general management and supervision of a performance."@en .

<http://rdaregistry.info/Elements/e/P20032>
    rdakit:instructionNumber "18.5" ;
    rdakit:toolkitDefinition "An agent contributing to an expression of a work by acting as an interviewer, reporter, pollster, or some other information gathering agent."@en, "Personne, famille ou collectivité contribuant à une expression d’une œuvre en agissant à titre d’intervieweur, de journaliste, de sondeur ou d’autre agent recueillant de l’information."@fr, "Una persona, familia o entidad corporativa que contribuye a una expresión de una obra actuando como entrevistador, reportero, encuestador, o algún otro agente recolector de información."@es ;
    rdakit:toolkitLabel "entrevistador (expresión)"@es, "interviewer (expression)"@en, "intervieweur (expression)"@fr ;
    reg:hasSubproperty <http://rdaregistry.info/Elements/e/object/P20032> ;
    reg:hasUnconstrained <http://rdaregistry.info/Elements/u/P60430> ;
    reg:lexicalAlias <http://rdaregistry.info/Elements/e/interviewerExpression.en> ;
    reg:name "interviewerExpression"@en ;
    reg:status <http://metadataregistry.org/uri/RegStatus/1001> ;
    a rdf:Property ;
    rdfs:domain <http://rdaregistry.info/Elements/c/C10006> ;
    rdfs:isDefinedBy <http://rdaregistry.info/Elements/e/> ;
    rdfs:label "has interviewer (expression)"@en ;
    rdfs:subPropertyOf <http://rdaregistry.info/Elements/e/P20053> ;
    skos:definition "Relates an expression to an agent contributing to an expression of a work by acting as an interviewer, reporter, pollster, or some other information gathering agent."@en .

<http://rdaregistry.info/Elements/e/P20033>
    rdakit:instructionNumber "18.5" ;
    rdakit:toolkitDefinition "An agent contributing to an expression of a work by an architect, inventor, etc., by making detailed plans or drawings for buildings, ships, aircraft, machines, objects, etc."@en, "Personne, famille ou collectivité contribuant à une expression d’une œuvre par un architecte, un inventeur, etc. en effectuant des plans ou des dessins détaillés pour des bâtiments, des navires, des avions, des machines, des objets, etc."@fr, "Una persona, familia o entidad corporativa que contribuye a una expresión de una obra de un arquitecto, inventor, etc., haciendo planos o dibujos detallados de edificios, barcos, aviones, máquinas, objetos, etc."@es ;
    rdakit:toolkitLabel "dessinateur industriel"@fr, "dibujante"@es, "draftsman"@en ;
    reg:hasSubproperty <http://rdaregistry.info/Elements/e/object/P20033> ;
    reg:hasUnconstrained <http://rdaregistry.info/Elements/u/P60381> ;
    reg:lexicalAlias <http://rdaregistry.info/Elements/e/draftsman.en> ;
    reg:name "draftsman"@en ;
    reg:status <http://metadataregistry.org/uri/RegStatus/1001> ;
    a rdf:Property ;
    rdfs:domain <http://rdaregistry.info/Elements/c/C10006> ;
    rdfs:isDefinedBy <http://rdaregistry.info/Elements/e/> ;
    rdfs:label "has draftsman"@en ;
    rdfs:subPropertyOf <http://rdaregistry.info/Elements/e/P20053> ;
    skos:definition "Relates an expression to an agent contributing to an expression of a work by an architect, inventor, etc., by making detailed plans or drawings for buildings, ships, aircraft, machines, objects, etc."@en .

<http://rdaregistry.info/Elements/e/P20034>
    rdakit:instructionNumber "18.5" ;
    rdakit:seeAlso <http://rdaregistry.info/Elements/e/P20029> ;
    rdakit:toolkitDefinition "An agent contributing to an expression of a work by writing down or notating unwritten or unnotated content, or by changing it from one system of notation to another."@en, "Personne, famille ou collectivité contribuant à une expression d’une œuvre en écrivant ou en notant un contenu auparavant non écrit ou non noté, ou bien en le transposant d’un système de notation à un autre."@fr, "Una persona, familia o entidad corporativa que contribuye a una expresión de una obra mediante la escritura o notación de contenido no escrito o no notado, o cambiando de un sistema de notación a otro."@es ;
    rdakit:toolkitLabel "transcriber"@en, "transcripteur"@fr, "transcriptor"@es ;
    reg:hasSubproperty <http://rdaregistry.info/Elements/e/object/P20034> ;
    reg:hasUnconstrained <http://rdaregistry.info/Elements/u/P60382> ;
    reg:lexicalAlias <http://rdaregistry.info/Elements/e/transcriber.en> ;
    reg:name "transcriber"@en ;
    reg:status <http://metadataregistry.org/uri/RegStatus/1001> ;
    a rdf:Property ;
    rdfs:domain <http://rdaregistry.info/Elements/c/C10006> ;
    rdfs:isDefinedBy <http://rdaregistry.info/Elements/e/> ;
    rdfs:label "has transcriber"@en ;
    rdfs:subPropertyOf <http://rdaregistry.info/Elements/e/P20053> ;
    skos:definition "Relates an expression to an agent contributing to an expression of a work by writing down or notating unwritten or unnotated content, or by changing it from one system of notation to another."@en ;
    skos:scopeNote "Transcription of a musical work for a different instrument or performing group is excluded."@en .

<http://rdaregistry.info/Elements/e/P20035>
    rdakit:instructionNumber "18.5" ;
    rdakit:toolkitDefinition "An agent contributing to an expression of a work by coordinating the activities of composers, sound editors, and sound mixers for a moving image production or for a musical or dramatic presentation or entertainment."@en, "Personne, famille ou collectivité contribuant à une expression d’une œuvre en coordonnant les activités du compositeur, du monteur son et des mixeurs de son pour une production d’images animées ou bien pour une représentation ou un spectacle dramatique ou musical."@fr, "Una persona, familia o entidad corporativa que contribuye a una expresión de una obra coordinando las actividades del compositor, el editor de sonido, y los mezcladores de sonido para una producción de una imagen en movimiento o para una producción teatral, musical o un espectáculo."@es ;
    rdakit:toolkitLabel "directeur musical"@fr, "director musical"@es, "musical director"@en ;
    reg:hasSubproperty <http://rdaregistry.info/Elements/e/object/P20035> ;
    reg:hasUnconstrained <http://rdaregistry.info/Elements/u/P60383> ;
    reg:lexicalAlias <http://rdaregistry.info/Elements/e/musicalDirector.en> ;
    reg:name "musicalDirector"@en ;
    reg:status <http://metadataregistry.org/uri/RegStatus/1001> ;
    a rdf:Property ;
    rdfs:domain <http://rdaregistry.info/Elements/c/C10006> ;
    rdfs:isDefinedBy <http://rdaregistry.info/Elements/e/> ;
    rdfs:label "has musical director"@en ;
    rdfs:subPropertyOf <http://rdaregistry.info/Elements/e/P20053> ;
    skos:definition "Relates an expression to an agent contributing to an expression of a work by coordinating the activities of composers, sound editors, and sound mixers for a moving image production or for a musical or dramatic presentation or entertainment."@en .

<http://rdaregistry.info/Elements/e/P20036>
    rdakit:instructionNumber "18.5" ;
    rdakit:toolkitDefinition "An agent contributing to an expression of a work by designing costumes for a moving image production or for a musical or dramatic presentation or entertainment."@en, "Personne, famille ou collectivité contribuant à une expression d’une œuvre en créant les costumes pour une production d’images animées ou bien pour une représentation ou un spectacle musical ou dramatique."@fr, "Una persona, familia o entidad corporativa que contribuye a una expresión de una obra diseñando el vestuario para una producción de una imagen en movimiento o para una producción teatral o musical o un espectáculo."@es ;
    rdakit:toolkitLabel "costume designer"@en, "créateur de costumes"@fr, "diseñador de vestuario"@es ;
    reg:hasSubproperty <http://rdaregistry.info/Elements/e/object/P20036> ;
    reg:hasUnconstrained <http://rdaregistry.info/Elements/u/P60384> ;
    reg:lexicalAlias <http://rdaregistry.info/Elements/e/costumeDesigner.en> ;
    reg:name "costumeDesigner"@en ;
    reg:status <http://metadataregistry.org/uri/RegStatus/1001> ;
    a rdf:Property ;
    rdfs:domain <http://rdaregistry.info/Elements/c/C10006> ;
    rdfs:isDefinedBy <http://rdaregistry.info/Elements/e/> ;
    rdfs:label "has costume designer"@en ;
    rdfs:subPropertyOf <http://rdaregistry.info/Elements/e/P20053> ;
    skos:definition "Relates an expression to an agent contributing to an expression of a work by designing costumes for a moving image production or for a musical or dramatic presentation or entertainment."@en .

<http://rdaregistry.info/Elements/e/P20037>
    rdakit:instructionNumber "18.5" ;
    rdakit:toolkitDefinition "An agent contributing to an expression of a work by expressing the linguistic content of the work in a language different from that of previous expressions of the original work."@en, "Personne, famille ou collectivité contribuant à une expression d’une œuvre en exprimant le texte original de l’œuvre dans une langue différente de celle de l’œuvre originale."@fr, "Una persona, familia o entidad corporativa que contribuye a una expresión de una obra expresando el contenido linguístico de la obra en una lengua diferente de las expresiones previas de la obra."@es ;
    rdakit:toolkitLabel "traducteur"@fr, "traductor"@es, "translator"@en ;
    reg:hasSubproperty <http://rdaregistry.info/Elements/e/object/P20037> ;
    reg:hasUnconstrained <http://rdaregistry.info/Elements/u/P60385> ;
    reg:lexicalAlias <http://rdaregistry.info/Elements/e/translator.en> ;
    reg:name "translator"@en ;
    reg:status <http://metadataregistry.org/uri/RegStatus/1001> ;
    a rdf:Property ;
    rdfs:domain <http://rdaregistry.info/Elements/c/C10006> ;
    rdfs:isDefinedBy <http://rdaregistry.info/Elements/e/> ;
    rdfs:label "has translator"@en ;
    rdfs:subPropertyOf <http://rdaregistry.info/Elements/e/P20053> ;
    skos:definition "Relates an expression to an agent contributing to an expression of a work by expressing the linguistic content of the work in a language different from that of previous expressions of the original work."@en ;
    skos:scopeNote "Translation of linguistic content between forms of the same language from different time periods is included."@en .

<http://rdaregistry.info/Elements/e/P20038>
    rdakit:instructionNumber "18.5" ;
    rdakit:toolkitDefinition "An agent contributing to an expression of a work by overseeing artists and craftspeople who build sets for moving image productions."@en, "Personne, famille ou collectivité contribuant à une expression d’une œuvre en supervisant les artistes et les artisans qui construisent les décors pour des productions d’images animées."@fr, "Una persona, familia o entidad corporativa que contribuye a una expresión de una obra supervisando los artistas y obreros que construyen los platos para producciones de imágenes en movimiento."@es ;
    rdakit:toolkitLabel "art director"@en, "directeur artistique"@fr, "director artístico"@es ;
    reg:hasSubproperty <http://rdaregistry.info/Elements/e/object/P20038> ;
    reg:hasUnconstrained <http://rdaregistry.info/Elements/u/P60386> ;
    reg:lexicalAlias <http://rdaregistry.info/Elements/e/artDirector.en> ;
    reg:name "artDirector"@en ;
    reg:status <http://metadataregistry.org/uri/RegStatus/1001> ;
    a rdf:Property ;
    rdfs:domain <http://rdaregistry.info/Elements/c/C10006> ;
    rdfs:isDefinedBy <http://rdaregistry.info/Elements/e/> ;
    rdfs:label "has art director"@en ;
    rdfs:subPropertyOf <http://rdaregistry.info/Elements/e/P20053> ;
    skos:definition "Relates an expression to an agent contributing to an expression of a work by overseeing artists and craftspeople who build sets for moving image productions."@en .

<http://rdaregistry.info/Elements/e/P20039>
    rdakit:instructionNumber "18.5" ;
    rdakit:toolkitDefinition "An agent contributing to an expression of a work by performing music, acting, dancing, speaking, etc., often in a musical or dramatic presentation, etc."@en, "Personne, famille ou collectivité contribuant à une expression d’une œuvre en exécutant de la musique, en jouant, en dansant, en parlant, etc. souvent dans une représentation musicale ou dramatique, etc."@fr, "Una persona, familia o entidad corporativa que contribuye a una expresión de una obra interpretando música, actuando, danzando, hablando, etc., generalmente en una producción musical o teatral, etc."@es ;
    rdakit:toolkitLabel "interprète"@fr, "intérprete"@es, "performer"@en ;
    reg:hasSubproperty <http://rdaregistry.info/Elements/e/P20011>, <http://rdaregistry.info/Elements/e/P20012>, <http://rdaregistry.info/Elements/e/P20013>, <http://rdaregistry.info/Elements/e/P20014>, <http://rdaregistry.info/Elements/e/P20015>, <http://rdaregistry.info/Elements/e/P20016>, <http://rdaregistry.info/Elements/e/P20017>, <http://rdaregistry.info/Elements/e/P20018>, <http://rdaregistry.info/Elements/e/P20019>, <http://rdaregistry.info/Elements/e/P20020>, <http://rdaregistry.info/Elements/e/P20021>, <http://rdaregistry.info/Elements/e/P20022>, <http://rdaregistry.info/Elements/e/P20023>, <http://rdaregistry.info/Elements/e/P20024>, <http://rdaregistry.info/Elements/e/P20025>, <http://rdaregistry.info/Elements/e/object/P20039> ;
    reg:hasUnconstrained <http://rdaregistry.info/Elements/u/P60387> ;
    reg:lexicalAlias <http://rdaregistry.info/Elements/e/performer.en> ;
    reg:name "performer"@en ;
    reg:status <http://metadataregistry.org/uri/RegStatus/1001> ;
    a rdf:Property ;
    rdfs:domain <http://rdaregistry.info/Elements/c/C10006> ;
    rdfs:isDefinedBy <http://rdaregistry.info/Elements/e/> ;
    rdfs:label "has performer"@en ;
    rdfs:subPropertyOf <http://rdaregistry.info/Elements/e/P20053> ;
    skos:definition "Relates an expression to an agent contributing to an expression of a work by performing music, acting, dancing, speaking, etc., often in a musical or dramatic presentation, etc."@en .

<http://rdaregistry.info/Elements/e/P20040>
    rdakit:instructionNumber "18.5" ;
    rdakit:toolkitDefinition "An agent contributing to an expression of a work by preparing a court's opinions for publication."@en, "Personne, famille ou collectivité contribuant à une expression d’une œuvre en préparant les opinions d’un tribunal aux fins de publication."@fr, "Una persona, familia o entidad corporativa que contribuye a una expresión de una obra preparando las opiniones del tribunal para publicación."@es ;
    rdakit:toolkitLabel "court reporter"@en, "rapporteur judiciaire"@fr, "relator del tribunal"@es ;
    reg:hasSubproperty <http://rdaregistry.info/Elements/e/object/P20040> ;
    reg:hasUnconstrained <http://rdaregistry.info/Elements/u/P60388> ;
    reg:lexicalAlias <http://rdaregistry.info/Elements/e/courtReporter.en> ;
    reg:name "courtReporter"@en ;
    reg:status <http://metadataregistry.org/uri/RegStatus/1001> ;
    a rdf:Property ;
    rdfs:domain <http://rdaregistry.info/Elements/c/C10006> ;
    rdfs:isDefinedBy <http://rdaregistry.info/Elements/e/> ;
    rdfs:label "has court reporter"@en ;
    rdfs:subPropertyOf <http://rdaregistry.info/Elements/e/P20053> ;
    skos:definition "Relates an expression to an agent contributing to an expression of a work by preparing a court's opinions for publication."@en .

<http://rdaregistry.info/Elements/e/P20041>
    rdakit:instructionNumber "18.5" ;
    rdakit:toolkitDefinition "An agent contributing to an expression of a work by providing a preface to an original work."@en, "Personne, famille ou collectivité contribuant à une expression d’une œuvre en fournissant une préface à l’œuvre originale."@fr, "Una persona, familia o entidad corporativa que contribuye a una expresión de una obra ofreciendo un prefacio a la obra original."@es ;
    rdakit:toolkitLabel "autor de prefacio"@es, "préfacier"@fr, "writer of preface"@en ;
    reg:hasSubproperty <http://rdaregistry.info/Elements/e/object/P20041> ;
    reg:hasUnconstrained <http://rdaregistry.info/Elements/u/P60389> ;
    reg:lexicalAlias <http://rdaregistry.info/Elements/e/writerOfPreface.en> ;
    reg:name "writerOfPreface"@en ;
    reg:status <http://metadataregistry.org/uri/RegStatus/1001> ;
    a rdf:Property ;
    rdfs:domain <http://rdaregistry.info/Elements/c/C10006> ;
    rdfs:isDefinedBy <http://rdaregistry.info/Elements/e/> ;
    rdfs:label "has writer of preface"@en ;
    rdfs:subPropertyOf <http://rdaregistry.info/Elements/e/P20046> ;
    skos:definition "Relates an expression to an agent contributing to an expression of a work by providing a preface to an original work."@en .

<http://rdaregistry.info/Elements/e/P20042>
    rdakit:instructionNumber "18.5" ;
    rdakit:toolkitDefinition "An agent contributing to an expression of a work by providing additional cartography, or by modifying previous cartography."@en, "Personne, famille ou collectivité contribuant à une expression d’une œuvre en fournissant une cartographie additionnelle ou en modifiant la cartographie antérieure."@fr, "Una persona, familia o entidad corporativa que contribuye a una expresión de una obra proporcionando cartografía adicional o modificando la cartografía anterior."@es ;
    rdakit:toolkitLabel "cartographe (expression)"@fr, "cartographer (expression)"@en, "cartógrafo (expresión)"@es ;
    reg:hasSubproperty <http://rdaregistry.info/Elements/e/object/P20042> ;
    reg:hasUnconstrained <http://rdaregistry.info/Elements/u/P60425> ;
    reg:lexicalAlias <http://rdaregistry.info/Elements/e/cartographerExpression.en> ;
    reg:name "cartographerExpression"@en ;
    reg:status <http://metadataregistry.org/uri/RegStatus/1001> ;
    a rdf:Property ;
    rdfs:domain <http://rdaregistry.info/Elements/c/C10006> ;
    rdfs:isDefinedBy <http://rdaregistry.info/Elements/e/> ;
    rdfs:label "has cartographer (expression)"@en ;
    rdfs:subPropertyOf <http://rdaregistry.info/Elements/e/P20053> ;
    skos:definition "Relates an expression to an agent contributing to an expression of a work by providing additional cartography, or by modifying previous cartography."@en .

<http://rdaregistry.info/Elements/e/P20043>
    rdakit:instructionNumber "18.5" ;
    rdakit:toolkitDefinition "An agent contributing to an expression of a work by providing additional choreography, or by modifying previous choreography."@en, "Personne, famille ou collectivité contribuant à une expression d’une œuvre en fournissant une chorégraphie additionnelle ou en modifiant la chorégraphie antérieure."@fr, "Una persona, familia o entidad corporativa que contribuye a una expresión de una obra proporcionando coreografía adicional, o modificando la coreografía anterior."@es ;
    rdakit:toolkitLabel "choreographer (expression)"@en, "chorégraphe (expression)"@fr, "coreógrafo (expresión)"@es ;
    reg:hasSubproperty <http://rdaregistry.info/Elements/e/object/P20043> ;
    reg:hasUnconstrained <http://rdaregistry.info/Elements/u/P60433> ;
    reg:lexicalAlias <http://rdaregistry.info/Elements/e/choreographerExpression.en> ;
    reg:name "choreographerExpression"@en ;
    reg:status <http://metadataregistry.org/uri/RegStatus/1001> ;
    a rdf:Property ;
    rdfs:domain <http://rdaregistry.info/Elements/c/C10006> ;
    rdfs:isDefinedBy <http://rdaregistry.info/Elements/e/> ;
    rdfs:label "has choreographer (expression)"@en ;
    rdfs:subPropertyOf <http://rdaregistry.info/Elements/e/P20053> ;
    skos:definition "Relates an expression to an agent contributing to an expression of a work by providing additional choreography, or by modifying previous choreography."@en .

<http://rdaregistry.info/Elements/e/P20044>
    rdakit:instructionNumber "18.5" ;
    rdakit:toolkitDefinition "An agent contributing to an expression of a work by providing an interpretation or critical explanation of an original work."@en, "Personne, famille ou collectivité contribuant à une expression d’une œuvre en fournissant une interprétation ou une critique de l’œuvre originale."@fr, "Una persona, familia o entidad corporativa que contribuye a una expresión de una obra ofreciendo una interpretación o explicación crítica de la obra original."@es ;
    rdakit:toolkitLabel "auteur de commentaire ajouté"@fr, "autor de comentario adicional"@es, "writer of added commentary"@en ;
    reg:hasSubproperty <http://rdaregistry.info/Elements/e/object/P20044> ;
    reg:hasUnconstrained <http://rdaregistry.info/Elements/u/P60390> ;
    reg:lexicalAlias <http://rdaregistry.info/Elements/e/writerOfAddedCommentary.en> ;
    reg:name "writerOfAddedCommentary"@en ;
    reg:status <http://metadataregistry.org/uri/RegStatus/1001> ;
    a rdf:Property ;
    rdfs:domain <http://rdaregistry.info/Elements/c/C10006> ;
    rdfs:isDefinedBy <http://rdaregistry.info/Elements/e/> ;
    rdfs:label "has writer of added commentary"@en ;
    rdfs:subPropertyOf <http://rdaregistry.info/Elements/e/P20046> ;
    skos:definition "Relates an expression to an agent contributing to an expression of a work by providing an interpretation or critical explanation of an original work."@en .

<http://rdaregistry.info/Elements/e/P20045>
    rdakit:instructionNumber "18.5" ;
    rdakit:toolkitDefinition "An agent contributing to an expression of a work by providing an introduction to an original work."@en, "Personne, famille ou collectivité contribuant à une expression d’une œuvre en fournissant une introduction à l’œuvre originale."@fr, "Una persona, familia o entidad corporativa que contribuye a una expresión de una obra ofreciendo una introducción a la obra original."@es ;
    rdakit:toolkitLabel "auteur d’introduction"@fr, "autor de introducción"@es, "writer of introduction"@en ;
    reg:hasSubproperty <http://rdaregistry.info/Elements/e/object/P20045> ;
    reg:hasUnconstrained <http://rdaregistry.info/Elements/u/P60391> ;
    reg:lexicalAlias <http://rdaregistry.info/Elements/e/writerOfIntroduction.en> ;
    reg:name "writerOfIntroduction"@en ;
    reg:status <http://metadataregistry.org/uri/RegStatus/1001> ;
    a rdf:Property ;
    rdfs:domain <http://rdaregistry.info/Elements/c/C10006> ;
    rdfs:isDefinedBy <http://rdaregistry.info/Elements/e/> ;
    rdfs:label "has writer of introduction"@en ;
    rdfs:subPropertyOf <http://rdaregistry.info/Elements/e/P20046> ;
    skos:definition "Relates an expression to an agent contributing to an expression of a work by providing an introduction to an original work."@en .

<http://rdaregistry.info/Elements/e/P20046>
    rdakit:instructionNumber "18.5" ;
    rdakit:toolkitDefinition "An agent contributing to an expression of a work by providing supplementary textual content, such as an introduction or a preface, to an original work."@en, "Personne, famille ou collectivité contribuant à une expression d’une œuvre en fournissant du contenu textuel supplémentaire (par exemple, une introduction, une préface) à l’œuvre originale."@fr, "Una persona, familia o entidad corporativa que contribuye a una expresión de una obra ofreciendo contenido textual suplementario (por ej., una introducción, un prefacio) a la obra original."@es ;
    rdakit:toolkitLabel "auteur de contenu textuel supplémentaire"@fr, "autor de contenido textual suplementario"@es, "writer of supplementary textual content"@en ;
    reg:hasSubproperty <http://rdaregistry.info/Elements/e/P20030>, <http://rdaregistry.info/Elements/e/P20041>, <http://rdaregistry.info/Elements/e/P20044>, <http://rdaregistry.info/Elements/e/P20045>, <http://rdaregistry.info/Elements/e/P20275>, <http://rdaregistry.info/Elements/e/object/P20046> ;
    reg:hasUnconstrained <http://rdaregistry.info/Elements/u/P60392> ;
    reg:lexicalAlias <http://rdaregistry.info/Elements/e/writerOfSupplementaryTextualContent.en> ;
    reg:name "writerOfSupplementaryTextualContent"@en ;
    reg:status <http://metadataregistry.org/uri/RegStatus/1001> ;
    a rdf:Property ;
    rdfs:domain <http://rdaregistry.info/Elements/c/C10006> ;
    rdfs:isDefinedBy <http://rdaregistry.info/Elements/e/> ;
    rdfs:label "has writer of supplementary textual content"@en ;
    rdfs:subPropertyOf <http://rdaregistry.info/Elements/e/P20053> ;
    skos:definition "Relates an expression to an agent contributing to an expression of a work by providing supplementary textual content, such as an introduction or a preface, to an original work."@en .

<http://rdaregistry.info/Elements/e/P20047>
    rdakit:instructionNumber "18.5" ;
    rdakit:toolkitDefinition "An agent contributing to an expression of a work by responding to an interviewer, usually a reporter, pollster, or some other information gathering agent."@en, "Personne, famille ou collectivité contribuant à une expression d’une œuvre en répondant à un intervieweur, habituellement un journaliste, un sondeur ou un autre agent recueillant de l’information."@fr, "Una persona, familia o entidad corporativa que contribuye a una expresión de una obra respondiendo a un entrevistador, generalmente un reportero, encuestador, o algún otro agente recolector de información."@es ;
    rdakit:toolkitLabel "entrevistado (expresión)"@es, "interviewee (expression)"@en, "interviewé (expression)"@fr ;
    reg:hasSubproperty <http://rdaregistry.info/Elements/e/object/P20047> ;
    reg:hasUnconstrained <http://rdaregistry.info/Elements/u/P60432> ;
    reg:lexicalAlias <http://rdaregistry.info/Elements/e/intervieweeExpression.en> ;
    reg:name "intervieweeExpression"@en ;
    reg:status <http://metadataregistry.org/uri/RegStatus/1001> ;
    a rdf:Property ;
    rdfs:domain <http://rdaregistry.info/Elements/c/C10006> ;
    rdfs:isDefinedBy <http://rdaregistry.info/Elements/e/> ;
    rdfs:label "has interviewee (expression)"@en ;
    rdfs:subPropertyOf <http://rdaregistry.info/Elements/e/P20053> ;
    skos:definition "Relates an expression to an agent contributing to an expression of a work by responding to an interviewer, usually a reporter, pollster, or some other information gathering agent."@en .

<http://rdaregistry.info/Elements/e/P20048>
    rdakit:instructionNumber "18.5" ;
    rdakit:seeAlso <http://rdaregistry.info/Elements/w/P10061> ;
    rdakit:toolkitDefinition "An agent contributing to an expression of a work by revising or clarifying the content, or by selecting and putting together works, or parts of works, by one or more creators."@en, "Personne, famille ou collectivité contribuant à une expression d’une œuvre en révisant ou en clarifiant le contenu, ou bien en choisissant et en rassemblant des œuvres, ou des parties d’œuvres, d’un ou de plusieurs créateurs."@fr, "Una persona, familia o entidad corporativa que contribuye a una expresión de una obra revisando o aclarando el contenido, por ej., agregando una introducción, notas u otro material crítico."@es ;
    rdakit:toolkitLabel "editor"@en, "editor"@es, "éditeur intellectuel"@fr ;
    reg:hasSubproperty <http://rdaregistry.info/Elements/e/object/P20048> ;
    reg:hasUnconstrained <http://rdaregistry.info/Elements/u/P60393> ;
    reg:lexicalAlias <http://rdaregistry.info/Elements/e/editor.en> ;
    reg:name "editor"@en ;
    reg:status <http://metadataregistry.org/uri/RegStatus/1001> ;
    a rdf:Property ;
    rdfs:domain <http://rdaregistry.info/Elements/c/C10006> ;
    rdfs:isDefinedBy <http://rdaregistry.info/Elements/e/> ;
    rdfs:label "has editor"@en ;
    rdfs:subPropertyOf <http://rdaregistry.info/Elements/e/P20053> ;
    skos:definition "Relates an expression to an agent contributing to an expression of a work by revising or clarifying the content, or by selecting and putting together works, or parts of works, by one or more creators."@en ;
    skos:scopeNote "Addition of an introduction, notes, or other critical matter, or preparing an expression of a work for production, publication, or distribution is included. Major revision, adaptation, etc., that substantially changes the nature and content of the original work, resulting in a new work, is excluded."@en .

<http://rdaregistry.info/Elements/e/P20049>
    rdakit:instructionNumber "18.5" ;
    rdakit:seeAlso <http://rdaregistry.info/Elements/w/P10061> ;
    rdakit:toolkitDefinition "An agent contributing to an expression of a work by shortening or condensing an original work but leaving the nature and content substantially unchanged."@en, "Personne, famille ou collectivité contribuant à une expression d’une œuvre en abrégeant ou en condensant l’œuvre originale tout en conservant la nature et le contenu de l’œuvre originale sensiblement inchangés."@fr, "Una persona, familia o entidad corporativa que contribuye a una expresión de una obra acortando o condensando la obra original pero dejando intacta la naturaleza y el contenido de la obra original."@es ;
    rdakit:toolkitLabel "abridger"@en, "abréviateur"@fr, "responsable de la edición abreviada/abreviador"@es ;
    reg:hasSubproperty <http://rdaregistry.info/Elements/e/object/P20049> ;
    reg:hasUnconstrained <http://rdaregistry.info/Elements/u/P60394> ;
    reg:lexicalAlias <http://rdaregistry.info/Elements/e/abridger.en> ;
    reg:name "abridger"@en ;
    reg:status <http://metadataregistry.org/uri/RegStatus/1001> ;
    a rdf:Property ;
    rdfs:domain <http://rdaregistry.info/Elements/c/C10006> ;
    rdfs:isDefinedBy <http://rdaregistry.info/Elements/e/> ;
    rdfs:label "has abridger"@en ;
    rdfs:subPropertyOf <http://rdaregistry.info/Elements/e/P20053> ;
    skos:definition "Relates an expression to an agent contributing to an expression of a work by shortening or condensing an original work but leaving the nature and content substantially unchanged."@en ;
    skos:scopeNote "Substantial modification that results in the creation of a new work is excluded."@en .

<http://rdaregistry.info/Elements/e/P20050>
    rdakit:instructionNumber "18.5" ;
    rdakit:toolkitDefinition "An audio engineer contributing to the audio content of an expression by supervising the technical aspects of a recording session."@en, "Personne, famille ou collectivité contribuant à une expression d’une œuvre en supervisant les aspects techniques d’une séance d’enregistrement sonore ou vidéo."@fr, "Una persona, familia o entidad corporativa que contribuye a una expresión de una obra supervisando los aspectos técnicos de una sesión de grabación de sonido o video."@es ;
    rdakit:toolkitLabel "ingeniero de grabación"@es, "ingénieur du son"@fr, "recording engineer"@en ;
    reg:hasSubproperty <http://rdaregistry.info/Elements/e/object/P20050> ;
    reg:hasUnconstrained <http://rdaregistry.info/Elements/u/P60395> ;
    reg:lexicalAlias <http://rdaregistry.info/Elements/e/recordingEngineer.en> ;
    reg:name "recordingEngineer"@en ;
    reg:status <http://metadataregistry.org/uri/RegStatus/1001> ;
    a rdf:Property ;
    rdfs:domain <http://rdaregistry.info/Elements/c/C10006> ;
    rdfs:isDefinedBy <http://rdaregistry.info/Elements/e/> ;
    rdfs:label "has recording engineer"@en ;
    rdfs:subPropertyOf <http://rdaregistry.info/Elements/e/P20292> ;
    skos:definition "Relates an expression to an audio engineer contributing to the audio content of an expression by supervising the technical aspects of a recording session."@en .

<http://rdaregistry.info/Elements/e/P20051>
    rdakit:instructionNumber "18.5" ;
    rdakit:seeAlso <http://rdaregistry.info/Elements/w/P10058> ;
    rdakit:toolkitDefinition "An agent contributing to an expression of a work by supplementing the primary content with drawings, diagrams, photographs, etc."@en, "Personne, famille ou collectivité contribuant à une expression d’une œuvre en complétant le contenu principal avec des dessins, des diagrammes, des photographies, etc."@fr, "Una persona, familia o entidad corporativa que contribuye a una expresión de una obra complementando el contenido primario con dibujos, diagramas, fotografías, etc."@es ;
    rdakit:toolkitLabel "illustrateur"@fr, "illustrator"@en, "ilustrador"@es ;
    reg:hasSubproperty <http://rdaregistry.info/Elements/e/P20259>, <http://rdaregistry.info/Elements/e/P20288>, <http://rdaregistry.info/Elements/e/object/P20051> ;
    reg:hasUnconstrained <http://rdaregistry.info/Elements/u/P60396> ;
    reg:lexicalAlias <http://rdaregistry.info/Elements/e/illustrator.en> ;
    reg:name "illustrator"@en ;
    reg:status <http://metadataregistry.org/uri/RegStatus/1001> ;
    a rdf:Property ;
    rdfs:domain <http://rdaregistry.info/Elements/c/C10006> ;
    rdfs:isDefinedBy <http://rdaregistry.info/Elements/e/> ;
    rdfs:label "has illustrator"@en ;
    rdfs:subPropertyOf <http://rdaregistry.info/Elements/e/P20053> ;
    skos:definition "Relates an expression to an agent contributing to an expression of a work by supplementing the primary content with drawings, diagrams, photographs, etc."@en ;
    skos:scopeNote "Creation of content that is primarily artistic is excluded."@en .

<http://rdaregistry.info/Elements/e/P20052>
    rdakit:instructionNumber "18.5" ;
    rdakit:toolkitDefinition "An agent contributing to an expression of a work by using a recording device to capture sound and/or video during a recording session, including field recordings of natural sounds, folkloric events, music, etc."@en, "Personne, famille ou collectivité contribuant à une expression d’une œuvre en utilisant un appareil d’enregistrement pour capter le son et/ou la vidéo durant une séance d’enregistrement, y compris les enregistrements de terrain de sons naturels, de prestations folkloriques, de musique, etc."@fr, "Una persona, familia o entidad corporativa que contribuye a una expresión de una obra utilizando un mecanismo de grabación para capturar sonido y/o video durante una sesión de grabación, incluyendo grabación de sonidos naturales, eventos folclóricos, música, etc."@es ;
    rdakit:toolkitLabel "opérateur d’enregistrement"@fr, "recordist"@en, "técnico de grabación"@es ;
    reg:hasSubproperty <http://rdaregistry.info/Elements/e/object/P20052> ;
    reg:hasUnconstrained <http://rdaregistry.info/Elements/u/P60397> ;
    reg:lexicalAlias <http://rdaregistry.info/Elements/e/recordist.en> ;
    reg:name "recordist"@en ;
    reg:status <http://metadataregistry.org/uri/RegStatus/1001> ;
    a rdf:Property ;
    rdfs:domain <http://rdaregistry.info/Elements/c/C10006> ;
    rdfs:isDefinedBy <http://rdaregistry.info/Elements/e/> ;
    rdfs:label "has recordist"@en ;
    rdfs:subPropertyOf <http://rdaregistry.info/Elements/e/P20053> ;
    skos:definition "Relates an expression to an agent contributing to an expression of a work by using a recording device to capture sound and/or video during a recording session, including field recordings of natural sounds, folkloric events, music, etc."@en .

<http://rdaregistry.info/Elements/e/P20053>
    rdakit:instructionNumber "20.2" ;
    rdakit:toolkitDefinition "An agent contributing to an expression."@en, "Personne, famille ou collectivité contribuant à une expression."@fr, "Una persona, familia o entidad corporativa que contribuye a  una expresión."@es ;
    rdakit:toolkitLabel "bidragsgivare"@sv, "colaborador"@es, "contributeur"@fr, "contributor"@en ;
    reg:hasSubproperty <http://rdaregistry.info/Elements/e/P20026>, <http://rdaregistry.info/Elements/e/P20027>, <http://rdaregistry.info/Elements/e/P20028>, <http://rdaregistry.info/Elements/e/P20029>, <http://rdaregistry.info/Elements/e/P20031>, <http://rdaregistry.info/Elements/e/P20032>, <http://rdaregistry.info/Elements/e/P20033>, <http://rdaregistry.info/Elements/e/P20034>, <http://rdaregistry.info/Elements/e/P20035>, <http://rdaregistry.info/Elements/e/P20036>, <http://rdaregistry.info/Elements/e/P20037>, <http://rdaregistry.info/Elements/e/P20038>, <http://rdaregistry.info/Elements/e/P20039>, <http://rdaregistry.info/Elements/e/P20040>, <http://rdaregistry.info/Elements/e/P20042>, <http://rdaregistry.info/Elements/e/P20043>, <http://rdaregistry.info/Elements/e/P20046>, <http://rdaregistry.info/Elements/e/P20047>, <http://rdaregistry.info/Elements/e/P20048>, <http://rdaregistry.info/Elements/e/P20049>, <http://rdaregistry.info/Elements/e/P20050>, <http://rdaregistry.info/Elements/e/P20051>, <http://rdaregistry.info/Elements/e/P20052>, <http://rdaregistry.info/Elements/e/P20054>, <http://rdaregistry.info/Elements/e/P20055>, <http://rdaregistry.info/Elements/e/P20056>, <http://rdaregistry.info/Elements/e/P20058>, <http://rdaregistry.info/Elements/e/P20257>, <http://rdaregistry.info/Elements/e/P20258>, <http://rdaregistry.info/Elements/e/P20276>, <http://rdaregistry.info/Elements/e/P20277>, <http://rdaregistry.info/Elements/e/P20279>, <http://rdaregistry.info/Elements/e/P20280>, <http://rdaregistry.info/Elements/e/P20283>, <http://rdaregistry.info/Elements/e/P20284>, <http://rdaregistry.info/Elements/e/P20287>, <http://rdaregistry.info/Elements/e/P20289>, <http://rdaregistry.info/Elements/e/P20292>, <http://rdaregistry.info/Elements/e/P20294>, <http://rdaregistry.info/Elements/e/P20295>, <http://rdaregistry.info/Elements/e/P20296>, <http://rdaregistry.info/Elements/e/object/P20053> ;
    reg:hasUnconstrained <http://rdaregistry.info/Elements/u/P60398> ;
    reg:lexicalAlias <http://rdaregistry.info/Elements/e/contributor.en> ;
    reg:name "contributor"@en ;
    reg:status <http://metadataregistry.org/uri/RegStatus/1001> ;
    a rdf:Property ;
    rdfs:domain <http://rdaregistry.info/Elements/c/C10006> ;
    rdfs:isDefinedBy <http://rdaregistry.info/Elements/e/> ;
    rdfs:label "har bidragsgivare"@sv, "has contributor"@en ;
    rdfs:subPropertyOf <http://rdaregistry.info/Elements/e/P20301> ;
    skos:definition "Relates an expression to an agent contributing to an expression."@en ;
    skos:scopeNote "Contributors include editors, translators, arrangers of music, performers, etc."@en .

<http://rdaregistry.info/Elements/e/P20054>
    rdakit:instructionNumber "18.5" ;
    rdakit:toolkitDefinition "An agent mentioned in an \"X presents:\" credit for moving image materials and who is probably associated with production, finance, or distribution in some way."@en, "Personne, famille ou collectivité mentionnée dans un générique d’images animées sous la forme « X présente » et qui est probablement associée d’une façon quelconque à la production, au financement ou à la distribution."@fr, "Un intérprete que contribuye a una expresión de una obra dirigiendo un programa (a menudo una transmisión) que incluye otros invitados, intérpretes, etc., (por ej., presentadores de programas de debates).  "@es ;
    rdakit:toolkitLabel "presentador"@es, "presenter"@en, "présentateur"@fr ;
    reg:hasSubproperty <http://rdaregistry.info/Elements/e/object/P20054> ;
    reg:hasUnconstrained <http://rdaregistry.info/Elements/u/P60419> ;
    reg:lexicalAlias <http://rdaregistry.info/Elements/e/presenter.en> ;
    reg:name "presenter"@en ;
    reg:status <http://metadataregistry.org/uri/RegStatus/1001> ;
    a rdf:Property ;
    rdfs:domain <http://rdaregistry.info/Elements/c/C10006> ;
    rdfs:isDefinedBy <http://rdaregistry.info/Elements/e/> ;
    rdfs:label "has presenter"@en ;
    rdfs:subPropertyOf <http://rdaregistry.info/Elements/e/P20053> ;
    skos:definition "Relates an expression to an agent mentioned in an \"X presents:\" credit for moving image materials and who is probably associated with production, finance, or distribution in some way."@en .

<http://rdaregistry.info/Elements/e/P20055>
    rdakit:instructionNumber "18.5" ;
    rdakit:toolkitDefinition "An agent responsible for assembling, arranging, and trimming film, video, or other moving image formats, including both visual and audio aspects."@en, "Personne, famille ou collectivité responsable de l’assemblage, de l’arrangement et du découpage de film, de vidéo ou d’autres formats d’images animées, y compris les aspects visuels et sonores."@fr, "Una persona, familia o entidad corporativa responsable de unir, componer y recortar película cinematográfica, video u otros formatos de imágenes en movimiento, incluyendo tanto aspectos visuales como de sonido."@es ;
    rdakit:toolkitLabel "editor of moving image work"@en, "montador"@es, "monteur d’œuvre d’images animées"@fr ;
    reg:hasSubproperty <http://rdaregistry.info/Elements/e/object/P20055> ;
    reg:hasUnconstrained <http://rdaregistry.info/Elements/u/P60422> ;
    reg:lexicalAlias <http://rdaregistry.info/Elements/e/editorOfMovingImageWork.en> ;
    reg:name "editorOfMovingImageWork"@en ;
    reg:status <http://metadataregistry.org/uri/RegStatus/1001> ;
    a rdf:Property ;
    rdfs:domain <http://rdaregistry.info/Elements/c/C10006> ;
    rdfs:isDefinedBy <http://rdaregistry.info/Elements/e/> ;
    rdfs:label "has editor of moving image work"@en ;
    rdfs:subPropertyOf <http://rdaregistry.info/Elements/e/P20053> ;
    skos:definition "Relates an expression to an agent responsible for assembling, arranging, and trimming film, video, or other moving image formats, including both visual and audio aspects."@en .

<http://rdaregistry.info/Elements/e/P20056>
    rdakit:instructionNumber "18.5" ;
    rdakit:toolkitDefinition "An agent responsible for designing the overall visual appearance of a moving image production."@en, "Personne, famille ou collectivité responsable de concevoir l’aspect visuel global d’une production d’images animées."@fr, "Una persona, familia o entidad corporativa responsable del diseño de la apariencia visual general de una producción de una imagen en movimiento."@es ;
    rdakit:toolkitLabel "chef décorateur"@fr, "diseñador de producción"@es, "production designer"@en ;
    reg:hasSubproperty <http://rdaregistry.info/Elements/e/object/P20056> ;
    reg:hasUnconstrained <http://rdaregistry.info/Elements/u/P60437> ;
    reg:lexicalAlias <http://rdaregistry.info/Elements/e/productionDesigner.en> ;
    reg:name "productionDesigner"@en ;
    reg:status <http://metadataregistry.org/uri/RegStatus/1001> ;
    a rdf:Property ;
    rdfs:domain <http://rdaregistry.info/Elements/c/C10006> ;
    rdfs:isDefinedBy <http://rdaregistry.info/Elements/e/> ;
    rdfs:label "has production designer"@en ;
    rdfs:subPropertyOf <http://rdaregistry.info/Elements/e/P20053> ;
    skos:definition "Relates an expression to an agent responsible for designing the overall visual appearance of a moving image production."@en .

<http://rdaregistry.info/Elements/e/P20057>
    reg:status <http://metadataregistry.org/uri/RegStatus/1008> ;
    a rdf:Property ;
    rdfs:isDefinedBy <http://rdaregistry.info/Elements/e/> .

<http://rdaregistry.info/Elements/e/P20058>
    rdakit:instructionNumber "18.5" ;
    rdakit:toolkitDefinition "An agent responsible for recording the minutes of a meeting."@en, "Personne, famille ou collectivité responsable de rédiger le procès-verbal d’une réunion."@fr, "Una persona, familia o entidad corporativa responsable de registrar las actas de una reunión."@es ;
    rdakit:toolkitLabel "minute taker"@en, "procès-verbaliste"@fr, "secretario de actas"@es ;
    reg:hasSubproperty <http://rdaregistry.info/Elements/e/object/P20058> ;
    reg:hasUnconstrained <http://rdaregistry.info/Elements/u/P60446> ;
    reg:lexicalAlias <http://rdaregistry.info/Elements/e/minuteTaker.en> ;
    reg:name "minuteTaker"@en ;
    reg:status <http://metadataregistry.org/uri/RegStatus/1001> ;
    a rdf:Property ;
    rdfs:domain <http://rdaregistry.info/Elements/c/C10006> ;
    rdfs:isDefinedBy <http://rdaregistry.info/Elements/e/> ;
    rdfs:label "has minute taker"@en ;
    rdfs:subPropertyOf <http://rdaregistry.info/Elements/e/P20053> ;
    skos:definition "Relates an expression to an agent responsible for recording the minutes of a meeting."@en .

<http://rdaregistry.info/Elements/e/P20059>
    rdakit:instructionNumber "17.9" ;
    rdakit:toolkitDefinition "A physical embodiment of an expression."@en, "Matérialisation d’une expression."@fr, "Una materialización física de una expresión."@es ;
    rdakit:toolkitLabel "manifestación de la expresión"@es, "manifestation av uttryck"@sv, "manifestation d’une expression"@fr, "manifestation of expression"@en ;
    reg:hasSubproperty <http://rdaregistry.info/Elements/e/object/P20059> ;
    reg:lexicalAlias <http://rdaregistry.info/Elements/e/manifestationOfExpression.en> ;
    reg:name "manifestationOfExpression"@en ;
    reg:status <http://metadataregistry.org/uri/RegStatus/1001> ;
    a rdf:Property ;
    rdfs:domain <http://rdaregistry.info/Elements/c/C10006> ;
    rdfs:isDefinedBy <http://rdaregistry.info/Elements/e/> ;
    rdfs:label "har manifestation av uttryck"@sv, "has manifestation of expression"@en ;
    skos:definition "Relates an expression to a physical embodiment of an expression."@en .

<http://rdaregistry.info/Elements/e/P20060>
    rdakit:instructionNumber "24.5" ;
    rdakit:toolkitDefinition "A radio program based on a source expression."@en, "Un programa de radio basado en la expresión fuente."@es, "Émission de radio basée sur l’expression source."@fr ;
    rdakit:toolkitLabel "adaptada como programa de radio (expresión)"@es, "adapted as radio program (expression)"@en, "adapté en émission de radio (expression)"@fr ;
    reg:hasSubproperty <http://rdaregistry.info/Elements/e/object/P20060> ;
    reg:hasUnconstrained <http://rdaregistry.info/Elements/u/P60174> ;
    reg:lexicalAlias <http://rdaregistry.info/Elements/e/adaptedAsRadioProgramExpression.en> ;
    reg:name "adaptedAsRadioProgramExpression"@en ;
    reg:status <http://metadataregistry.org/uri/RegStatus/1001> ;
    a rdf:Property ;
    rdfs:domain <http://rdaregistry.info/Elements/c/C10006> ;
    rdfs:isDefinedBy <http://rdaregistry.info/Elements/e/> ;
    rdfs:label "is adapted as radio program (expression)"@en ;
    rdfs:subPropertyOf <http://rdaregistry.info/Elements/e/P20153> ;
    skos:definition "Relates an expression to a radio program based on a source expression."@en .

<http://rdaregistry.info/Elements/e/P20061>
    rdakit:instructionNumber "7.13.4" ;
    rdakit:toolkitDefinition "A set of characters or symbols used to express the content of an expression in a form that can be perceived through touch."@en, "Ensemble de signes et/ou de symboles utilisés pour exprimer le contenu d’une ressource sous une forme perceptible au toucher."@fr, "Un conjunto de caracteres y/o símbolos utilizados para expresar el contenido de un recurso en tal forma que se pueda percibir mediante el tacto."@es ;
    rdakit:toolkitLabel "form av taktil notation"@sv, "form of tactile notation"@en, "forma de notación táctil"@es, "forme de la notation tactile"@fr ;
    reg:hasUnconstrained <http://rdaregistry.info/Elements/u/P60318> ;
    reg:lexicalAlias <http://rdaregistry.info/Elements/e/formOfTactileNotation.en> ;
    reg:name "formOfTactileNotation"@en ;
    reg:status <http://metadataregistry.org/uri/RegStatus/1001> ;
    a rdf:Property ;
    rdfs:domain <http://rdaregistry.info/Elements/c/C10006> ;
    rdfs:isDefinedBy <http://rdaregistry.info/Elements/e/> ;
    rdfs:label "har form av taktil notation"@sv, "has form of tactile notation"@en ;
    rdfs:subPropertyOf <http://rdaregistry.info/Elements/e/P20062> ;
    skos:definition "Relates an expression to a set of characters or symbols used to express the content of an expression in a form that can be perceived through touch."@en .

<http://rdaregistry.info/Elements/e/P20062>
    rdakit:instructionNumber "7.13" ;
    rdakit:toolkitDefinition "A set of characters or symbols used to express the content of an expression."@en, "Ensemble de signes et/ou de symboles utilisés pour exprimer le contenu d’une ressource."@fr, "Un conjunto de caracteres y/o símbolos utilizados para expresar el contenido de un recurso."@es ;
    rdakit:toolkitLabel "form av notation"@sv, "form of notation"@en, "forma de notación"@es, "forme de la notation"@fr ;
    reg:hasSubproperty <http://rdaregistry.info/Elements/e/P20061>, <http://rdaregistry.info/Elements/e/P20063>, <http://rdaregistry.info/Elements/e/P20064>, <http://rdaregistry.info/Elements/e/P20065> ;
    reg:hasUnconstrained <http://rdaregistry.info/Elements/u/P60319> ;
    reg:lexicalAlias <http://rdaregistry.info/Elements/e/formOfNotation.en> ;
    reg:name "formOfNotation"@en ;
    reg:status <http://metadataregistry.org/uri/RegStatus/1001> ;
    a rdf:Property ;
    rdfs:domain <http://rdaregistry.info/Elements/c/C10006> ;
    rdfs:isDefinedBy <http://rdaregistry.info/Elements/e/> ;
    rdfs:label "har form av notation"@sv, "has form of notation"@en ;
    skos:definition "Relates an expression to a set of characters or symbols used to express the content of an expression."@en .

<http://rdaregistry.info/Elements/e/P20063>
    rdakit:instructionNumber "7.13.5" ;
    rdakit:toolkitDefinition "A set of characters or symbols used to express movement content of an expression."@en, "Ensemble de signes et/ou de caractères utilisés pour exprimer le contenu du mouvement d’une ressource."@fr, "Un conjunto de caracteres y/o símbolos usados para expresar el contenido de movimientos de un recurso."@es ;
    rdakit:toolkitLabel "form of notated movement"@en, "forma de notación de movimientos"@es, "forme de la notation du mouvement"@fr ;
    reg:hasUnconstrained <http://rdaregistry.info/Elements/u/P60320> ;
    reg:lexicalAlias <http://rdaregistry.info/Elements/e/formOfNotatedMovement.en> ;
    reg:name "formOfNotatedMovement"@en ;
    reg:status <http://metadataregistry.org/uri/RegStatus/1001> ;
    a rdf:Property ;
    rdfs:domain <http://rdaregistry.info/Elements/c/C10006> ;
    rdfs:isDefinedBy <http://rdaregistry.info/Elements/e/> ;
    rdfs:label "has form of notated movement"@en ;
    rdfs:subPropertyOf <http://rdaregistry.info/Elements/e/P20062> ;
    skos:definition "Relates an expression to a set of characters or symbols used to express movement content of an expression."@en .

<http://rdaregistry.info/Elements/e/P20064>
    rdakit:instructionNumber "7.13.3" ;
    rdakit:toolkitDefinition "A set of characters or symbols used to express musical content of an expression."@en, "Ensemble de signes et/ou de symboles utilisés pour exprimer le contenu musical d’une ressource"@fr, "Un conjunto de caracteres y/o símbolos utilizados para expresar el contenido musical de un recurso."@es ;
    rdakit:toolkitLabel "form av musiknotation"@sv, "form of musical notation"@en, "forma de la notación musical"@es, "forme de la notation musicale"@fr ;
    reg:hasUnconstrained <http://rdaregistry.info/Elements/u/P60321> ;
    reg:lexicalAlias <http://rdaregistry.info/Elements/e/formOfMusicalNotation.en> ;
    reg:name "formOfMusicalNotation"@en ;
    reg:status <http://metadataregistry.org/uri/RegStatus/1001> ;
    a rdf:Property ;
    rdfs:domain <http://rdaregistry.info/Elements/c/C10006> ;
    rdfs:isDefinedBy <http://rdaregistry.info/Elements/e/> ;
    rdfs:label "har form av musiknotation"@sv, "has form of musical notation"@en ;
    rdfs:subPropertyOf <http://rdaregistry.info/Elements/e/P20062> ;
    skos:definition "Relates an expression to a set of characters or symbols used to express musical content of an expression."@en .

<http://rdaregistry.info/Elements/e/P20065>
    rdakit:instructionNumber "7.13.2" ;
    rdakit:toolkitDefinition "A set of characters and/or symbols used to express written language content of an expression."@en, "Ensemble de caractères et/ou de symboles utilisé pour exprimer le contenu linguistique écrit d’une ressource."@fr, "Un conjunto de caracteres y/o símbolos utilizados para expresar en lengua escrita el contenido de un recurso."@es ;
    rdakit:toolkitLabel "escritura"@es, "script"@en, "écriture"@fr ;
    reg:hasUnconstrained <http://rdaregistry.info/Elements/u/P60322> ;
    reg:lexicalAlias <http://rdaregistry.info/Elements/e/script.en> ;
    reg:name "script"@en ;
    reg:status <http://metadataregistry.org/uri/RegStatus/1001> ;
    a rdf:Property ;
    rdfs:domain <http://rdaregistry.info/Elements/c/C10006> ;
    rdfs:isDefinedBy <http://rdaregistry.info/Elements/e/> ;
    rdfs:label "has script"@en ;
    rdfs:subPropertyOf <http://rdaregistry.info/Elements/e/P20062> ;
    skos:definition "Relates an expression to a set of characters or symbols used to express written language content of an expression."@en .

<http://rdaregistry.info/Elements/e/P20066>
    rdakit:instructionNumber "24.5" ;
    rdakit:toolkitDefinition "A television program based on a source expression."@en, "Un programa de televisión basado en la expresión fuente."@es, "Émission de télévision basée sur l’expression source."@fr ;
    rdakit:toolkitLabel "adaptada como programa de televisión (expresión)"@es, "adapted as television program (expression)"@en, "adapté en émission de télévision (expression)"@fr ;
    reg:hasSubproperty <http://rdaregistry.info/Elements/e/object/P20066> ;
    reg:hasUnconstrained <http://rdaregistry.info/Elements/u/P60354> ;
    reg:lexicalAlias <http://rdaregistry.info/Elements/e/adaptedAsTelevisionProgramExpression.en> ;
    reg:name "adaptedAsTelevisionProgramExpression"@en ;
    reg:status <http://metadataregistry.org/uri/RegStatus/1001> ;
    a rdf:Property ;
    rdfs:domain <http://rdaregistry.info/Elements/c/C10006> ;
    rdfs:isDefinedBy <http://rdaregistry.info/Elements/e/> ;
    rdfs:label "is adapted as television program (expression)"@en ;
    rdfs:subPropertyOf <http://rdaregistry.info/Elements/e/P20153> ;
    skos:definition "Relates an expression to a television program based on a source expression."@en .

<http://rdaregistry.info/Elements/e/P20067>
    rdakit:instructionNumber "24.5" ;
    rdakit:toolkitDefinition "A video based on a source expression."@en, "Un video basado en la expresión fuente."@es, "Vidéo basée sur l’expression source."@fr ;
    rdakit:toolkitLabel "adaptada como video (expresión)"@es, "adapted as video (expression)"@en, "adapté en vidéo (expression)"@fr ;
    reg:hasSubproperty <http://rdaregistry.info/Elements/e/object/P20067> ;
    reg:hasUnconstrained <http://rdaregistry.info/Elements/u/P60361> ;
    reg:lexicalAlias <http://rdaregistry.info/Elements/e/adaptedAsVideoExpression.en> ;
    reg:name "adaptedAsVideoExpression"@en ;
    reg:status <http://metadataregistry.org/uri/RegStatus/1001> ;
    a rdf:Property ;
    rdfs:domain <http://rdaregistry.info/Elements/c/C10006> ;
    rdfs:isDefinedBy <http://rdaregistry.info/Elements/e/> ;
    rdfs:label "is adapted as video (expression)"@en ;
    rdfs:subPropertyOf <http://rdaregistry.info/Elements/e/P20153> ;
    skos:definition "Relates an expression to a video based on a source expression."@en .

<http://rdaregistry.info/Elements/e/P20068>
    rdakit:instructionNumber "18.5" ;
    rdakit:seeAlso <http://rdaregistry.info/Elements/w/P10204> ;
    rdakit:toolkitDefinition "A writer of words added to an expression of a musical work."@en, "Auteur de paroles ajoutées à une expression d’une œuvre musicale."@fr, "Un autor que agrega palabras a una expresión de una obra musical."@es ;
    rdakit:toolkitLabel "auteur de paroles ajoutées"@fr, "autor de letra adicional"@es, "writer of added lyrics"@en ;
    reg:hasSubproperty <http://rdaregistry.info/Elements/e/object/P20068> ;
    reg:hasUnconstrained <http://rdaregistry.info/Elements/u/P60371> ;
    reg:lexicalAlias <http://rdaregistry.info/Elements/e/writerOfAddedLyrics.en> ;
    reg:name "writerOfAddedLyrics"@en ;
    reg:status <http://metadataregistry.org/uri/RegStatus/1001> ;
    a rdf:Property ;
    rdfs:domain <http://rdaregistry.info/Elements/c/C10006> ;
    rdfs:isDefinedBy <http://rdaregistry.info/Elements/e/> ;
    rdfs:label "has writer of added lyrics"@en ;
    rdfs:subPropertyOf <http://rdaregistry.info/Elements/e/P20030> ;
    skos:definition "Relates an expression to a writer of words added to an expression of a musical work."@en ;
    skos:scopeNote "Writing of lyrics in collaboration with a composer to form an original work is excluded."@en .

<http://rdaregistry.info/Elements/e/P20069>
    rdakit:instructionNumber "7.10" ;
    rdakit:toolkitDefinition "An abstract, summary, synopsis, etc., of the content of an expression."@en, "Synthèse, résumé, synopsis, etc. du contenu d’une ressource."@fr, "Un resumen, sumario, sinopsis, etc., del contenido de un recurso."@es ;
    rdakit:toolkitLabel "innehållsbeskrivning"@sv, "resumen del contenido"@es, "résumé du contenu"@fr, "summarization of content"@en ;
    reg:hasUnconstrained <http://rdaregistry.info/Elements/u/P60372> ;
    reg:lexicalAlias <http://rdaregistry.info/Elements/e/summarizationOfContent.en> ;
    reg:name "summarizationOfContent"@en ;
    reg:status <http://metadataregistry.org/uri/RegStatus/1001> ;
    a rdf:Property ;
    rdfs:domain <http://rdaregistry.info/Elements/c/C10006> ;
    rdfs:isDefinedBy <http://rdaregistry.info/Elements/e/> ;
    rdfs:label "har innehållsbeskrivning"@sv, "has summarization of content"@en ;
    skos:definition "Relates an expression to an abstract, summary, synopsis, etc., of the content of an expression."@en .

<http://rdaregistry.info/Elements/e/P20070>
    rdakit:instructionNumber "18.5" ;
    rdakit:toolkitDefinition "Acteur contribuant à une expression d’une œuvre en prêtant sa voix à des personnages dans des productions radiophoniques et audio et à des personnages animés dans des œuvres d’images animées, de même qu’en prêtant sa voix hors champ dans des messages publicitaires à la radio et à la télévision, du doublage, etc."@fr, "An actor contributing to an expression of a work by providing the voice for characters in radio and audio productions and for animated characters in moving image works, as well as by providing voice-overs in radio and television commercials, dubbed resources, etc."@en, "Un actor que contribuye a una expresión de una obra proporcionando la voz de los personajes en radio y producciones de sonido y de personajes animados en obras de imágenes en movimiento, al igual que proporcionando voces sobrepuestas en comerciales de radio y televisión, recursos de doblaje, etc."@es ;
    rdakit:toolkitLabel "actor de voz"@es, "voice actor"@en, "voix"@fr ;
    reg:hasSubproperty <http://rdaregistry.info/Elements/e/object/P20070> ;
    reg:hasUnconstrained <http://rdaregistry.info/Elements/u/P60152> ;
    reg:lexicalAlias <http://rdaregistry.info/Elements/e/voiceActor.en> ;
    reg:name "voiceActor"@en ;
    reg:status <http://metadataregistry.org/uri/RegStatus/1001> ;
    a rdf:Property ;
    rdfs:domain <http://rdaregistry.info/Elements/c/C10006> ;
    rdfs:isDefinedBy <http://rdaregistry.info/Elements/e/> ;
    rdfs:label "has voice actor"@en ;
    rdfs:subPropertyOf <http://rdaregistry.info/Elements/e/P20012> ;
    skos:definition "Relates an expression to an actor contributing to an expression of a work by providing the voice for characters in radio and audio productions and for animated characters in moving image works, as well as by providing voice-overs in radio and television commercials, dubbed expressions, etc."@en .

<http://rdaregistry.info/Elements/e/P20071>
    rdakit:instructionNumber "7.29" ;
    rdakit:toolkitDefinition "A note providing additional information about content recorded as an expression attribute."@en, "Annotation fournissant un complément d’information relatif au contenu enregistré comme attribut de l’expression."@fr, "Una anotación que proporciona información adicional sobre contenido registrado como un atributo de la expresión."@es ;
    rdakit:toolkitLabel "nota sobre la expresión"@es, "note on expression"@en, "note relative à l’expression"@fr ;
    reg:hasSubproperty <http://rdaregistry.info/Elements/e/P20010> ;
    reg:hasUnconstrained <http://rdaregistry.info/Elements/u/P60470> ;
    reg:lexicalAlias <http://rdaregistry.info/Elements/e/noteOnExpression.en> ;
    reg:name "noteOnExpression"@en ;
    reg:status <http://metadataregistry.org/uri/RegStatus/1001> ;
    a rdf:Property ;
    rdfs:domain <http://rdaregistry.info/Elements/c/C10006> ;
    rdfs:isDefinedBy <http://rdaregistry.info/Elements/e/> ;
    rdfs:label "has note on expression"@en ;
    skos:definition "Relates an expression to a note providing additional information about content recorded as an expression attribute."@en .

<http://rdaregistry.info/Elements/e/P20072>
    reg:hasSubproperty <http://rdaregistry.info/Elements/e/P20136>, <http://rdaregistry.info/Elements/e/P20150>, <http://rdaregistry.info/Elements/e/P20178>, <http://rdaregistry.info/Elements/e/P20182>, <http://rdaregistry.info/Elements/e/P20187> ;
    reg:status <http://metadataregistry.org/uri/RegStatus/1008> ;
    a rdf:Property ;
    rdfs:isDefinedBy <http://rdaregistry.info/Elements/e/> ;
    rdfs:subPropertyOf <http://rdaregistry.info/Elements/e/P20234> .

<http://rdaregistry.info/Elements/e/P20073>
    rdakit:instructionNumber "24.5" ;
    rdakit:toolkitDefinition "An expression of a dramatic work adapted from a source expression."@en, "Expression d’une œuvre théâtrale adaptée de l’expression source."@fr, "Una expresión de una obra dramática adaptada de la expresión fuente."@es ;
    rdakit:toolkitLabel "adapté au théâtre comme (expression)"@fr, "dramatizada como (expresión)"@es, "dramatized as (expression)"@en ;
    reg:hasSubproperty <http://rdaregistry.info/Elements/e/object/P20073> ;
    reg:hasUnconstrained <http://rdaregistry.info/Elements/u/P60088> ;
    reg:lexicalAlias <http://rdaregistry.info/Elements/e/dramatizedAsExpression.en> ;
    reg:name "dramatizedAsExpression"@en ;
    reg:status <http://metadataregistry.org/uri/RegStatus/1001> ;
    a rdf:Property ;
    rdfs:domain <http://rdaregistry.info/Elements/c/C10006> ;
    rdfs:isDefinedBy <http://rdaregistry.info/Elements/e/> ;
    rdfs:label "is dramatized as (expression)"@en ;
    rdfs:subPropertyOf <http://rdaregistry.info/Elements/e/P20153> ;
    skos:definition "Relates an expression to an expression of a dramatic work adapted from a source expression."@en .

<http://rdaregistry.info/Elements/e/P20074>
    rdakit:instructionNumber "24.5" ;
    rdakit:toolkitDefinition "An expression of a larger work of which the expression is a discrete component."@en, "Expression d’une œuvre plus vaste dont l’expression est une composante distincte."@fr, "Una expresión de una obra mayor de la cual una parte es un componente separado."@es ;
    rdakit:toolkitLabel "contained in (expression)"@en, "contenida en (expresión)"@es, "contenu dans (expression)"@fr ;
    reg:hasSubproperty <http://rdaregistry.info/Elements/e/object/P20074> ;
    reg:hasUnconstrained <http://rdaregistry.info/Elements/u/P60101> ;
    reg:lexicalAlias <http://rdaregistry.info/Elements/e/containedInExpression.en> ;
    reg:name "containedInExpression"@en ;
    reg:status <http://metadataregistry.org/uri/RegStatus/1001> ;
    a rdf:Property ;
    rdfs:domain <http://rdaregistry.info/Elements/c/C10006> ;
    rdfs:isDefinedBy <http://rdaregistry.info/Elements/e/> ;
    rdfs:label "is contained in (expression)"@en ;
    rdfs:subPropertyOf <http://rdaregistry.info/Elements/e/P20236> ;
    skos:definition "Relates an expression to an expression of a larger work of which the expression is a discrete component."@en .

<http://rdaregistry.info/Elements/e/P20075>
    rdakit:instructionNumber "24.5" ;
    rdakit:toolkitDefinition "An expression of a later work used in part in place of an earlier expression usually because the later work contains updated or new information that makes part of the earlier expression obsolete."@en, "Expression d’une œuvre ultérieure utilisée en partie à la place d’une expression antérieure, généralement parce que l’œuvre ultérieure contient de l’information nouvelle ou mise à jour qui rend une partie de l’expression antérieure obsolète."@fr, "Una expresión de una obra anterior cuyo contenido ha sido reemplazado parcialmente por una expresión posterior, generalmente porque la obra posterior contiene información actualizada o nueva que hace obsoleta la expresión anterior."@es ;
    rdakit:toolkitLabel "reemplazo en parte de (expresión)"@es, "remplacé en partie par (expression)"@fr, "replaced in part by (expression)"@en ;
    reg:hasSubproperty <http://rdaregistry.info/Elements/e/object/P20075> ;
    reg:hasUnconstrained <http://rdaregistry.info/Elements/u/P60103> ;
    reg:lexicalAlias <http://rdaregistry.info/Elements/e/replacedInPartByExpression.en> ;
    reg:name "replacedInPartByExpression"@en ;
    reg:status <http://metadataregistry.org/uri/RegStatus/1001> ;
    a rdf:Property ;
    rdfs:domain <http://rdaregistry.info/Elements/c/C10006> ;
    rdfs:isDefinedBy <http://rdaregistry.info/Elements/e/> ;
    rdfs:label "is replaced in part by (expression)"@en ;
    rdfs:subPropertyOf <http://rdaregistry.info/Elements/e/P20169> ;
    skos:definition "Relates an expression to an expression of a later work used in part in place of an earlier expression usually because the later work contains updated or new information that makes part of the earlier expression obsolete."@en ;
    skos:scopeNote "This relationship applies generally to single-part units, multipart monographs, and integrating resources."@en .

<http://rdaregistry.info/Elements/e/P20076>
    rdakit:instructionNumber "24.5" ;
    rdakit:toolkitDefinition "An expression of a later work used in place of an earlier expression, usually because the later work contains updated or new information that makes the earlier expression obsolete."@en, "Expression d’une œuvre ultérieure utilisée à la place d’une expression antérieure, généralement parce que l’œuvre ultérieure contient de l’information nouvelle ou mise à jour qui rend l’expression antérieure obsolète."@fr, "Una expresión de una obra anterior cuyo contenido ha sido reemplazado por una expresión posterior, generalmente porque la obra posterior contiene información actualizada o nueva que hace obsoleta la expresión anterior."@es ;
    rdakit:toolkitLabel "reemplazo de (expresión)"@es, "remplacé par (expression)"@fr, "replaced by (expression)"@en ;
    reg:hasSubproperty <http://rdaregistry.info/Elements/e/object/P20076> ;
    reg:hasUnconstrained <http://rdaregistry.info/Elements/u/P60104> ;
    reg:lexicalAlias <http://rdaregistry.info/Elements/e/replacedByExpression.en> ;
    reg:name "replacedByExpression"@en ;
    reg:status <http://metadataregistry.org/uri/RegStatus/1001> ;
    a rdf:Property ;
    rdfs:domain <http://rdaregistry.info/Elements/c/C10006> ;
    rdfs:isDefinedBy <http://rdaregistry.info/Elements/e/> ;
    rdfs:label "is replaced by (expression)"@en ;
    rdfs:subPropertyOf <http://rdaregistry.info/Elements/e/P20169> ;
    skos:definition "Relates an expression to an expression of a later work used in place of an earlier expression, usually because the later work contains updated or new information that makes the earlier expression obsolete."@en ;
    skos:scopeNote "This relationship applies generally to single-part units, multipart monographs, and integrating resources."@en .

<http://rdaregistry.info/Elements/e/P20077>
    rdakit:instructionNumber "24.5" ;
    rdakit:toolkitDefinition "An expression of a literary composition in verse form adapted from a source expression."@en, "Expression d’une composition littéraire en vers adaptée de l’expression source."@fr, "Una expresión de una obra que fue adaptada como una composición literaria en forma de verso."@es ;
    rdakit:toolkitLabel "adaptación en verso de (expresión)"@es, "adapted in verse as (expression)"@en, "adapté en vers comme (expression)"@fr ;
    reg:hasSubproperty <http://rdaregistry.info/Elements/e/object/P20077> ;
    reg:hasUnconstrained <http://rdaregistry.info/Elements/u/P60106> ;
    reg:lexicalAlias <http://rdaregistry.info/Elements/e/adaptedInVerseAsExpression.en> ;
    reg:name "adaptedInVerseAsExpression"@en ;
    reg:status <http://metadataregistry.org/uri/RegStatus/1001> ;
    a rdf:Property ;
    rdfs:domain <http://rdaregistry.info/Elements/c/C10006> ;
    rdfs:isDefinedBy <http://rdaregistry.info/Elements/e/> ;
    rdfs:label "is adapted in verse as (expression)"@en ;
    rdfs:subPropertyOf <http://rdaregistry.info/Elements/e/P20153> ;
    skos:definition "Relates an expression to an expression of a literary composition in verse form adapted from a source expression."@en .

<http://rdaregistry.info/Elements/e/P20078>
    rdakit:instructionNumber "24.5" ;
    rdakit:toolkitDefinition "An expression of a moving image work in which spoken dialogue has been translated into a language different from that of the original work."@en, "Expression d’une œuvre d’images animées dans laquelle les dialogues parlés ont été traduits dans une langue différente de celle de l’œuvre d’origine."@fr, "Una expresión de una obra de imagen en movimiento en la cual el diálogo hablado se ha traducido a una lengua diferente de la de la obra original."@es ;
    rdakit:toolkitLabel "dubbed version of"@en, "version doublée de"@fr, "versión doblada de"@es ;
    reg:hasSubproperty <http://rdaregistry.info/Elements/e/object/P20078> ;
    reg:hasUnconstrained <http://rdaregistry.info/Elements/u/P60111> ;
    reg:lexicalAlias <http://rdaregistry.info/Elements/e/dubbedVersionOf.en> ;
    reg:name "dubbedVersionOf"@en ;
    reg:status <http://metadataregistry.org/uri/RegStatus/1001> ;
    a rdf:Property ;
    rdfs:domain <http://rdaregistry.info/Elements/c/C10006> ;
    rdfs:isDefinedBy <http://rdaregistry.info/Elements/e/> ;
    rdfs:label "is dubbed version of"@en ;
    rdfs:subPropertyOf <http://rdaregistry.info/Elements/e/P20141> ;
    skos:definition "Relates an expression to an expression of a moving image work in which spoken dialogue has been translated into a language different from that of the original work."@en .

<http://rdaregistry.info/Elements/e/P20079>
    rdakit:instructionNumber "24.5" ;
    rdakit:toolkitDefinition "An expression of a moving image work that translates spoken dialogue of the original work into a different language."@en, "Expression d’une œuvre d’images animées qui traduit les dialogues parlés de l’œuvre d’origine dans une langue différente."@fr, "Una expresión de una obra de imagen en movimiento que traduce el diálogo hablado de la obra original en una lengua diferente."@es ;
    rdakit:toolkitLabel "dubbed version"@en, "version doublée"@fr, "versión doblada"@es ;
    reg:hasSubproperty <http://rdaregistry.info/Elements/e/object/P20079> ;
    reg:hasUnconstrained <http://rdaregistry.info/Elements/u/P60112> ;
    reg:lexicalAlias <http://rdaregistry.info/Elements/e/dubbedVersion.en> ;
    reg:name "dubbedVersion"@en ;
    reg:status <http://metadataregistry.org/uri/RegStatus/1001> ;
    a rdf:Property ;
    rdfs:domain <http://rdaregistry.info/Elements/c/C10006> ;
    rdfs:isDefinedBy <http://rdaregistry.info/Elements/e/> ;
    rdfs:label "is dubbed version"@en ;
    rdfs:subPropertyOf <http://rdaregistry.info/Elements/e/P20171> ;
    skos:definition "Relates an expression to an expression of a moving image work that translates spoken dialogue of the original work into a different language."@en .

<http://rdaregistry.info/Elements/e/P20080>
    rdakit:instructionNumber "24.5" ;
    rdakit:toolkitDefinition "An expression of a musical work consisting of an ornamental passage for a soloist, added to a musical work such as a concerto, either by the same or a different composer."@en, "Expression d’une œuvre musicale consistant en un passage ornemental pour soliste, ajouté à une œuvre musicale telle qu’un concerto, soit par le même compositeur, soit par un compositeur différent."@fr, "Una expresión de una obra musical que consiste en un pasaje ornamental para un solista, añadida a una obra musical como un concierto, por igual o diferente compositor."@es ;
    rdakit:toolkitLabel "cadence (expression)"@fr, "cadencia (expresión)"@es, "cadenza (expression)"@en ;
    reg:hasSubproperty <http://rdaregistry.info/Elements/e/object/P20080> ;
    reg:hasUnconstrained <http://rdaregistry.info/Elements/u/P60113> ;
    reg:lexicalAlias <http://rdaregistry.info/Elements/e/cadenzaExpression.en> ;
    reg:name "cadenzaExpression"@en ;
    reg:status <http://metadataregistry.org/uri/RegStatus/1001> ;
    a rdf:Property ;
    rdfs:domain <http://rdaregistry.info/Elements/c/C10006> ;
    rdfs:isDefinedBy <http://rdaregistry.info/Elements/e/> ;
    rdfs:label "is cadenza (expression)"@en ;
    rdfs:subPropertyOf <http://rdaregistry.info/Elements/e/P20105> ;
    skos:definition "Relates an expression to an expression of a musical work consisting of an ornamental passage for a soloist, added to a musical work such as a concerto, either by the same or a different composer."@en .

<http://rdaregistry.info/Elements/e/P20081>
    rdakit:instructionNumber "24.5" ;
    rdakit:toolkitDefinition "An expression of a musical work from which melodic, thematic, or harmonic material is taken to form a discrete theme, which is repeated one or more times with subsequent modifications."@en, "Expression d’une œuvre musicale d’où est tirée de la matière mélodique, thématique ou harmonique pour former un thème distinct, qui est répété une ou plusieurs fois avec des modifications subséquentes."@fr, "Una expresión de una obra musical de la cual se toma el material melódico, temático o armónico para formar un tema separado, el cual es repetido una o más veces con modificaciones subsecuentes."@es ;
    rdakit:toolkitLabel "variaciones basadas en (expresión)"@es, "variations based on (expression)"@en, "variations basées sur (expression)"@fr ;
    reg:hasSubproperty <http://rdaregistry.info/Elements/e/object/P20081> ;
    reg:hasUnconstrained <http://rdaregistry.info/Elements/u/P60114> ;
    reg:lexicalAlias <http://rdaregistry.info/Elements/e/variationsBasedOnExpression.en> ;
    reg:name "variationsBasedOnExpression"@en ;
    reg:status <http://metadataregistry.org/uri/RegStatus/1001> ;
    a rdf:Property ;
    rdfs:domain <http://rdaregistry.info/Elements/c/C10006> ;
    rdfs:isDefinedBy <http://rdaregistry.info/Elements/e/> ;
    rdfs:label "is variations based on (expression)"@en ;
    rdfs:subPropertyOf <http://rdaregistry.info/Elements/e/P20204> ;
    skos:definition "Relates an expression to an expression of a musical work from which melodic, thematic, or harmonic material is taken to form a discrete theme, which is repeated one or more times with subsequent modifications."@en .

<http://rdaregistry.info/Elements/e/P20082>
    rdakit:instructionNumber "24.5" ;
    rdakit:toolkitDefinition "An expression of a musical work in which melodic, thematic, or harmonic material taken from a source work forms a discrete theme, which is repeated one or more times with subsequent modifications."@en, "Expression d’une œuvre musicale dans laquelle de la matière mélodique, thématique ou harmonique tirée de l’œuvre source forme un thème distinct qui est répété une ou plusieurs fois avec des modifications subséquentes."@fr, "Una expresión de una obra musical en la cual el material melódico, temático o harmónico se toma de la obra fuente para formar un tema separado, el cual se repite una o mas veces con las subsecuentes modificaciones."@es ;
    rdakit:toolkitLabel "modificada por variación como (expresión)"@es, "modified by variation as (expression)"@en, "modifié par variation comme (expression)"@fr ;
    reg:hasSubproperty <http://rdaregistry.info/Elements/e/object/P20082> ;
    reg:hasUnconstrained <http://rdaregistry.info/Elements/u/P60115> ;
    reg:lexicalAlias <http://rdaregistry.info/Elements/e/modifiedByVariationAsExpression.en> ;
    reg:name "modifiedByVariationAsExpression"@en ;
    reg:status <http://metadataregistry.org/uri/RegStatus/1001> ;
    a rdf:Property ;
    rdfs:domain <http://rdaregistry.info/Elements/c/C10006> ;
    rdfs:isDefinedBy <http://rdaregistry.info/Elements/e/> ;
    rdfs:label "is modified by variation as (expression)"@en ;
    rdfs:subPropertyOf <http://rdaregistry.info/Elements/e/P20203> ;
    skos:definition "Relates an expression to an expression of a musical work in which melodic, thematic, or harmonic material taken from a source work forms a discrete theme, which is repeated one or more times with subsequent modifications."@en .

<http://rdaregistry.info/Elements/e/P20083>
    rdakit:instructionNumber "24.5" ;
    rdakit:toolkitDefinition "An expression of a musical work such as a concerto for which an ornamental passage for a soloist has been composed, either by the same or a different composer."@en, "Expression d’une œuvre musicale telle qu’un concerto pour laquelle un passage ornemental pour soliste a été composé, soit par le même compositeur, soit par un compositeur différent."@fr, "Una expresión de una obra musical tal como un concierto para el cual se ha compuesto un pasaje ornamental para solista, ya sea por el mismo o diferente compositor."@es ;
    rdakit:toolkitLabel "cadence composée pour (expression)"@fr, "cadencia compuesta para (expresión)"@es, "cadenza composed for (expression)"@en ;
    reg:hasSubproperty <http://rdaregistry.info/Elements/e/object/P20083> ;
    reg:hasUnconstrained <http://rdaregistry.info/Elements/u/P60116> ;
    reg:lexicalAlias <http://rdaregistry.info/Elements/e/cadenzaComposedForExpression.en> ;
    reg:name "cadenzaComposedForExpression"@en ;
    reg:status <http://metadataregistry.org/uri/RegStatus/1001> ;
    a rdf:Property ;
    rdfs:domain <http://rdaregistry.info/Elements/c/C10006> ;
    rdfs:isDefinedBy <http://rdaregistry.info/Elements/e/> ;
    rdfs:label "is cadenza composed for (expression)"@en ;
    rdfs:subPropertyOf <http://rdaregistry.info/Elements/e/P20192> ;
    skos:definition "Relates an expression to an expression of a musical work such as a concerto for which an ornamental passage for a soloist has been composed, either by the same or a different composer."@en .

<http://rdaregistry.info/Elements/e/P20084>
    rdakit:instructionNumber "24.5" ;
    rdakit:toolkitDefinition "An expression of a musical work such as an opera or other work for the musical stage, or an oratorio, that uses the text of a related work."@en, "Expression d’une œuvre musicale telle qu’un opéra ou une autre œuvre pour la scène musicale, ou telle qu’un oratorio, qui utilise le texte de l’œuvre en relation."@fr, "Una expresión de una obra musical tal como una ópera u otra obra para representación musical, o un oratorio, que utiliza el texto de la obra relacionada."@es ;
    rdakit:toolkitLabel "libreto para (expresión)"@es, "libretto for (expression)"@en, "livret pour (expression)"@fr ;
    reg:hasSubproperty <http://rdaregistry.info/Elements/e/object/P20084> ;
    reg:hasUnconstrained <http://rdaregistry.info/Elements/u/P60117> ;
    reg:lexicalAlias <http://rdaregistry.info/Elements/e/librettoForExpression.en> ;
    reg:name "librettoForExpression"@en ;
    reg:status <http://metadataregistry.org/uri/RegStatus/1001> ;
    a rdf:Property ;
    rdfs:domain <http://rdaregistry.info/Elements/c/C10006> ;
    rdfs:isDefinedBy <http://rdaregistry.info/Elements/e/> ;
    rdfs:label "is libretto for (expression)"@en ;
    rdfs:subPropertyOf <http://rdaregistry.info/Elements/e/P20100> ;
    skos:definition "Relates an expression to an expression of a musical work such as an opera or other work for the musical stage, or an oratorio, that uses the text of a related work."@en .

<http://rdaregistry.info/Elements/e/P20085>
    rdakit:instructionNumber "24.5" ;
    rdakit:toolkitDefinition "An expression of a musical work that that provides incidental music for a play or other spoken work for the stage."@en, "Expression d’une œuvre musicale qui fournit la musique de scène pour une pièce de théâtre ou une autre œuvre parlée pour la scène."@fr, "Una expresión de una obra musical que proporciona la música incidental para una obra de teatro u otra obra hablada para el escenario."@es ;
    rdakit:toolkitLabel "incidental music (expression)"@en, "musique de scène (expression)"@fr, "música incidental (expresión)"@es ;
    reg:hasSubproperty <http://rdaregistry.info/Elements/e/object/P20085> ;
    reg:hasUnconstrained <http://rdaregistry.info/Elements/u/P60118> ;
    reg:lexicalAlias <http://rdaregistry.info/Elements/e/incidentalMusicExpression.en> ;
    reg:name "incidentalMusicExpression"@en ;
    reg:status <http://metadataregistry.org/uri/RegStatus/1001> ;
    a rdf:Property ;
    rdfs:domain <http://rdaregistry.info/Elements/c/C10006> ;
    rdfs:isDefinedBy <http://rdaregistry.info/Elements/e/> ;
    rdfs:label "is incidental music (expression)"@en ;
    rdfs:subPropertyOf <http://rdaregistry.info/Elements/e/P20243> ;
    skos:definition "Relates an expression to an expression of a musical work that that provides incidental music for a play or other spoken work for the stage."@en .

<http://rdaregistry.info/Elements/e/P20086>
    rdakit:instructionNumber "24.5" ;
    rdakit:toolkitDefinition "An expression of a new motion picture, radio program, television program, or video based on an earlier work."@en, "Expression d’un nouveau film, d’une nouvelle émission de radio, d’une nouvelle émission de télévision ou d’une nouvelle vidéo basée sur une œuvre antérieure."@fr, "Una expresión de una película cinematográfica, programa radial, programa de televisión o video nuevo basada en una obra anterior."@es ;
    rdakit:toolkitLabel "remade as (expression)"@en, "repris comme (expression)"@fr, "reproducida como (expresión)"@es ;
    reg:hasSubproperty <http://rdaregistry.info/Elements/e/object/P20086> ;
    reg:hasUnconstrained <http://rdaregistry.info/Elements/u/P60120> ;
    reg:lexicalAlias <http://rdaregistry.info/Elements/e/remadeAsExpression.en> ;
    reg:name "remadeAsExpression"@en ;
    reg:status <http://metadataregistry.org/uri/RegStatus/1001> ;
    a rdf:Property ;
    rdfs:domain <http://rdaregistry.info/Elements/c/C10006> ;
    rdfs:isDefinedBy <http://rdaregistry.info/Elements/e/> ;
    rdfs:label "is remade as (expression)"@en ;
    rdfs:subPropertyOf <http://rdaregistry.info/Elements/e/P20203> ;
    skos:definition "Relates an expression to an expression of a motion picture, radio program, television program, or video based on an earlier work."@en .

<http://rdaregistry.info/Elements/e/P20087>
    rdakit:instructionNumber "24.5" ;
    rdakit:toolkitDefinition "An expression of a non-dramatic musical work, other than an oratorio, that uses the text of a source work."@en, "Expression d’une œuvre musicale non théâtrale, autre qu’un oratorio, qui utilise le texte de l’œuvre source."@fr, "Una expresión de una obra musical no dramática, diferente de un oratorio, que usa el texto de la obra fuente."@es ;
    rdakit:toolkitLabel "hecha para música como (expresión)"@es, "mis en musique comme (expression)"@fr, "set to music as (expression)"@en ;
    reg:hasSubproperty <http://rdaregistry.info/Elements/e/object/P20087> ;
    reg:hasUnconstrained <http://rdaregistry.info/Elements/u/P60121> ;
    reg:lexicalAlias <http://rdaregistry.info/Elements/e/setToMusicAsExpression.en> ;
    reg:name "setToMusicAsExpression"@en ;
    reg:status <http://metadataregistry.org/uri/RegStatus/1001> ;
    a rdf:Property ;
    rdfs:domain <http://rdaregistry.info/Elements/c/C10006> ;
    rdfs:isDefinedBy <http://rdaregistry.info/Elements/e/> ;
    rdfs:label "is set to music as (expression)"@en ;
    rdfs:subPropertyOf <http://rdaregistry.info/Elements/e/P20203> ;
    skos:definition "Relates an expression to an expression of a non-dramatic musical work, other than an oratorio, that uses the text of a source work."@en .

<http://rdaregistry.info/Elements/e/P20088>
    rdakit:instructionNumber "24.5" ;
    rdakit:toolkitDefinition "An expression of a novel adapted from a source expression."@en, "Expression d’un roman adapté de l’expression source."@fr, "Una expresión de una novela adaptada de la expresión fuente."@es ;
    rdakit:toolkitLabel "adaptada como novela (expresión)"@es, "adapted as novel (expression)"@en, "adapté en roman (expression)"@fr ;
    reg:hasSubproperty <http://rdaregistry.info/Elements/e/object/P20088> ;
    reg:hasUnconstrained <http://rdaregistry.info/Elements/u/P60138> ;
    reg:lexicalAlias <http://rdaregistry.info/Elements/e/adaptedAsNovelExpression.en> ;
    reg:name "adaptedAsNovelExpression"@en ;
    reg:status <http://metadataregistry.org/uri/RegStatus/1001> ;
    a rdf:Property ;
    rdfs:domain <http://rdaregistry.info/Elements/c/C10006> ;
    rdfs:isDefinedBy <http://rdaregistry.info/Elements/e/> ;
    rdfs:label "is adapted as novel (expression)"@en ;
    rdfs:subPropertyOf <http://rdaregistry.info/Elements/e/P20153> ;
    skos:definition "Relates an expression to an expression of a novel adapted from a source expression."@en .

<http://rdaregistry.info/Elements/e/P20089>
    rdakit:instructionNumber "24.5" ;
    rdakit:toolkitDefinition "An expression of a work whose content is augmented with content from an expression of another work."@en, "Expression d’une œuvre prédominante qui est augmentée par une autre œuvre qui consiste en informations qui ne sont pas essentielles à la complétude du contenu, telles qu’une liste de références, des tableaux statistiques et des indications explicatives ; l’œuvre augmentante peut soit figurer à la fin du contenu, soit être publiée séparément."@fr, "Una expresión de una obra que es aumentada por otra obra que consiste en material que no es esencial para la integridad del contenido, tal como una lista de referencias, tablas estadísticas, material explicativo; la obra adicional puede venir al final del contenido, o ser publicada separadamente"@es ;
    rdakit:toolkitLabel "annexe de (expression)"@fr, "appendix to (expression)"@en, "apéndice de (expresión)"@es ;
    reg:hasSubproperty <http://rdaregistry.info/Elements/e/object/P20089> ;
    reg:hasUnconstrained <http://rdaregistry.info/Elements/u/P60253> ;
    reg:lexicalAlias <http://rdaregistry.info/Elements/e/appendixToExpression.en> ;
    reg:name "appendixToExpression"@en ;
    reg:status <http://metadataregistry.org/uri/RegStatus/1001> ;
    a rdf:Property ;
    rdfs:domain <http://rdaregistry.info/Elements/c/C10006> ;
    rdfs:isDefinedBy <http://rdaregistry.info/Elements/e/> ;
    rdfs:label "is appendix to (expression)"@en ;
    rdfs:subPropertyOf <http://rdaregistry.info/Elements/e/P20192> ;
    skos:definition "Relates an expression to an expression of a work whose content is augmented with content from an expression of another work."@en ;
    skos:scopeNote "Includes lists of references, statistical tables, and explanatory matter that are not essential to the completeness of the content."@en .

<http://rdaregistry.info/Elements/e/P20090>
    rdakit:instructionNumber "24.5" ;
    rdakit:toolkitDefinition "An expression of a work that is an abstracting and indexing service that abstracts the contents of a source expression."@en, "Expression d’une œuvre (service d’analyse et d’indexation) qui résume le contenu d’une expression source."@fr, "Una expresión de una obra (un servicio de indización y resúmenes) que resume el contenido de una expresión fuente."@es ;
    rdakit:toolkitLabel "abstracted in (expression)"@en, "resumida en (expresión)"@es, "résumé analytiquement dans (expression)"@fr ;
    reg:hasSubproperty <http://rdaregistry.info/Elements/e/object/P20090> ;
    reg:hasUnconstrained <http://rdaregistry.info/Elements/u/P60177> ;
    reg:lexicalAlias <http://rdaregistry.info/Elements/e/abstractedInExpression.en> ;
    reg:name "abstractedInExpression"@en ;
    reg:status <http://metadataregistry.org/uri/RegStatus/1001> ;
    a rdf:Property ;
    rdfs:domain <http://rdaregistry.info/Elements/c/C10006> ;
    rdfs:isDefinedBy <http://rdaregistry.info/Elements/e/> ;
    rdfs:label "is abstracted in (expression)"@en ;
    rdfs:subPropertyOf <http://rdaregistry.info/Elements/e/P20203> ;
    skos:definition "Relates an expression to an expression of a work that is an abstracting and indexing service that abstracts the contents of a source expression."@en .

<http://rdaregistry.info/Elements/e/P20091>
    rdakit:instructionNumber "24.5" ;
    rdakit:toolkitDefinition "An expression of a work that is an abstracting and indexing service that indexes the contents of a source expression."@en, "Expression d’une œuvre (service d’analyse et d’indexation) qui indexe le contenu d’une expression source."@fr, "Una expresión de una obra (un servicio de indización y resúmenes) que indiza el contenido de una expresión fuente."@es ;
    rdakit:toolkitLabel "indexed in (expression)"@en, "indexé dans (expression)"@fr, "indizada en (expresión)"@es ;
    reg:hasSubproperty <http://rdaregistry.info/Elements/e/object/P20091> ;
    reg:hasUnconstrained <http://rdaregistry.info/Elements/u/P60178> ;
    reg:lexicalAlias <http://rdaregistry.info/Elements/e/indexedInExpression.en> ;
    reg:name "indexedInExpression"@en ;
    reg:status <http://metadataregistry.org/uri/RegStatus/1001> ;
    a rdf:Property ;
    rdfs:domain <http://rdaregistry.info/Elements/c/C10006> ;
    rdfs:isDefinedBy <http://rdaregistry.info/Elements/e/> ;
    rdfs:label "is indexed in (expression)"@en ;
    rdfs:subPropertyOf <http://rdaregistry.info/Elements/e/P20203> ;
    skos:definition "Relates an expression to an expression of a work that is an abstracting and indexing service that indexes the contents of a source expression."@en .

<http://rdaregistry.info/Elements/e/P20092>
    rdakit:instructionNumber "24.5" ;
    rdakit:toolkitDefinition "An expression of a work consisting of movement based on a source work."@en, "Expression d’une œuvre consistant en mouvement (par exemple, de la danse) basée sur l’œuvre source."@fr, "Una expresión de una obra que consiste en movimiento (p. ej., danza) basada en la obra fuente."@es ;
    rdakit:toolkitLabel "adaptada como coreografía (expresión)"@es, "adapted as choreography (expression)"@en, "adapté en chorégraphie (expression)"@fr ;
    reg:hasSubproperty <http://rdaregistry.info/Elements/e/object/P20092> ;
    reg:hasUnconstrained <http://rdaregistry.info/Elements/u/P60180> ;
    reg:lexicalAlias <http://rdaregistry.info/Elements/e/adaptedAsChoreographyExpression.en> ;
    reg:name "adaptedAsChoreographyExpression"@en ;
    reg:status <http://metadataregistry.org/uri/RegStatus/1001> ;
    a rdf:Property ;
    rdfs:domain <http://rdaregistry.info/Elements/c/C10006> ;
    rdfs:isDefinedBy <http://rdaregistry.info/Elements/e/> ;
    rdfs:label "is adapted as choreography (expression)"@en ;
    rdfs:subPropertyOf <http://rdaregistry.info/Elements/e/P20153> ;
    skos:definition "Relates an expression to an expression of a work consisting of movement based on a source work."@en .

<http://rdaregistry.info/Elements/e/P20093>
    rdakit:instructionNumber "24.5" ;
    rdakit:toolkitDefinition "An expression of a work consisting of errors discovered after the publication of a predominant work, with their corrections."@en, "Expression d’une œuvre constituée des erreurs découvertes après la publication de l’œuvre prédominante, avec leurs corrections."@fr, "Una expresión de una obra que consiste en los errores descubiertos después de la publicación de la obra principal, con sus correcciones."@es ;
    rdakit:toolkitLabel "errata (expression)"@en, "errata (expression)"@fr, "fe de erratas (expresión)"@es ;
    reg:hasSubproperty <http://rdaregistry.info/Elements/e/object/P20093> ;
    reg:hasUnconstrained <http://rdaregistry.info/Elements/u/P60181> ;
    reg:lexicalAlias <http://rdaregistry.info/Elements/e/errataExpression.en> ;
    reg:name "errataExpression"@en ;
    reg:status <http://metadataregistry.org/uri/RegStatus/1001> ;
    a rdf:Property ;
    rdfs:domain <http://rdaregistry.info/Elements/c/C10006> ;
    rdfs:isDefinedBy <http://rdaregistry.info/Elements/e/> ;
    rdfs:label "is errata (expression)"@en ;
    rdfs:subPropertyOf <http://rdaregistry.info/Elements/e/P20105> ;
    skos:definition "Relates an expression to an expression of a work consisting of errors discovered after publication of a predominant work, with their corrections."@en .

<http://rdaregistry.info/Elements/e/P20094>
    rdakit:instructionNumber "24.5" ;
    rdakit:toolkitDefinition "An expression of a work consisting of pictorial content designed to explain or decorate an augmented expression."@en, "Expression d’une œuvre consistant en contenu visuel destiné à expliquer ou à décorer l’expression augmentée."@fr, "Una expresión de una obra que consiste en contenido pictórico diseñado para explicar o decorar la entidad aumentada."@es ;
    rdakit:toolkitLabel "illustrations (expression)"@en, "illustrations (expression)"@fr, "ilustraciones (expresión)"@es ;
    reg:hasSubproperty <http://rdaregistry.info/Elements/e/object/P20094> ;
    reg:hasUnconstrained <http://rdaregistry.info/Elements/u/P60182> ;
    reg:lexicalAlias <http://rdaregistry.info/Elements/e/illustrationsExpression.en> ;
    reg:name "illustrationsExpression"@en ;
    reg:status <http://metadataregistry.org/uri/RegStatus/1001> ;
    a rdf:Property ;
    rdfs:domain <http://rdaregistry.info/Elements/c/C10006> ;
    rdfs:isDefinedBy <http://rdaregistry.info/Elements/e/> ;
    rdfs:label "is illustrations (expression)"@en ;
    rdfs:subPropertyOf <http://rdaregistry.info/Elements/e/P20105> ;
    skos:definition "Relates an expression to an expression of a work consisting of pictorial content designed to explain or decorate an augmented expression."@en .

<http://rdaregistry.info/Elements/e/P20095>
    rdakit:instructionNumber "24.5" ;
    rdakit:toolkitDefinition "An expression of a work consisting of a screenplay for a motion picture, based on a source work."@en, "Expression d’une œuvre consistant en le scénario pour un film, basée sur l’œuvre source."@fr, "Una expresión de una obra que consiste en el guión para una película cinematográfica, basado en la obra fuente."@es ;
    rdakit:toolkitLabel "adaptada como guión cinematográfico (expresión)"@es, "adapted as motion picture screenplay (expression)"@en, "adapté en scénario de film (expression)"@fr ;
    reg:hasSubproperty <http://rdaregistry.info/Elements/e/object/P20095> ;
    reg:hasUnconstrained <http://rdaregistry.info/Elements/u/P60184> ;
    reg:lexicalAlias <http://rdaregistry.info/Elements/e/adaptedAsMotionPictureScreenplayExpression.en> ;
    reg:name "adaptedAsMotionPictureScreenplayExpression"@en ;
    reg:status <http://metadataregistry.org/uri/RegStatus/1001> ;
    a rdf:Property ;
    rdfs:domain <http://rdaregistry.info/Elements/c/C10006> ;
    rdfs:isDefinedBy <http://rdaregistry.info/Elements/e/> ;
    rdfs:label "is adapted as motion picture screenplay (expression)"@en ;
    rdfs:subPropertyOf <http://rdaregistry.info/Elements/e/P20096> ;
    skos:definition "Relates an expression to an expression of a work consisting of a screenplay for a motion picture, based on a source work."@en .

<http://rdaregistry.info/Elements/e/P20096>
    rdakit:instructionNumber "24.5" ;
    rdakit:toolkitDefinition "An expression of a work consisting of a screenplay for a motion picture, television program, or video, based on a source work."@en, "Expression d’une œuvre consistant en le scénario pour un film, une émission de télévision ou une vidéo, basée sur l’œuvre source."@fr, "Una expresión de una obra que consiste en el guión para una película cinematográfica, programa de televisión o video, basado en la obra fuente."@es ;
    rdakit:toolkitLabel "adaptada como guión (expresión)"@es, "adapted as screenplay (expression)"@en, "adapté en scénario (expression)"@fr ;
    reg:hasSubproperty <http://rdaregistry.info/Elements/e/P20095>, <http://rdaregistry.info/Elements/e/P20097>, <http://rdaregistry.info/Elements/e/P20098>, <http://rdaregistry.info/Elements/e/object/P20096> ;
    reg:hasUnconstrained <http://rdaregistry.info/Elements/u/P60185> ;
    reg:lexicalAlias <http://rdaregistry.info/Elements/e/adaptedAsScreenplayExpression.en> ;
    reg:name "adaptedAsScreenplayExpression"@en ;
    reg:status <http://metadataregistry.org/uri/RegStatus/1001> ;
    a rdf:Property ;
    rdfs:domain <http://rdaregistry.info/Elements/c/C10006> ;
    rdfs:isDefinedBy <http://rdaregistry.info/Elements/e/> ;
    rdfs:label "is adapted as screenplay (expression)"@en ;
    rdfs:subPropertyOf <http://rdaregistry.info/Elements/e/P20153> ;
    skos:definition "Relates an expression to an expression of a work consisting of a screenplay for a motion picture, television program, or video, based on a source work."@en .

<http://rdaregistry.info/Elements/e/P20097>
    rdakit:instructionNumber "24.5" ;
    rdakit:toolkitDefinition "An expression of a work consisting of a screenplay for a television program, based on a source work."@en, "Expression d’une œuvre consistant en le scénario pour une émission de télévision, basée sur l’œuvre source."@fr, "Una expresión de una obra que consiste en el guión para un programa de televisión, basado en la obra fuente."@es ;
    rdakit:toolkitLabel "adaptada como guión para televisión (expresión)"@es, "adapted as television screenplay (expression)"@en, "adapté en scénario de télévision (expression)"@fr ;
    reg:hasSubproperty <http://rdaregistry.info/Elements/e/object/P20097> ;
    reg:hasUnconstrained <http://rdaregistry.info/Elements/u/P60186> ;
    reg:lexicalAlias <http://rdaregistry.info/Elements/e/adaptedAsTelevisionScreenplayExpression.en> ;
    reg:name "adaptedAsTelevisionScreenplayExpression"@en ;
    reg:status <http://metadataregistry.org/uri/RegStatus/1001> ;
    a rdf:Property ;
    rdfs:domain <http://rdaregistry.info/Elements/c/C10006> ;
    rdfs:isDefinedBy <http://rdaregistry.info/Elements/e/> ;
    rdfs:label "is adapted as television screenplay (expression)"@en ;
    rdfs:subPropertyOf <http://rdaregistry.info/Elements/e/P20096> ;
    skos:definition "Relates an expression to an expression of a work consisting of a screenplay for a television program, based on a source work."@en .

<http://rdaregistry.info/Elements/e/P20098>
    rdakit:instructionNumber "24.5" ;
    rdakit:toolkitDefinition "An expression of a work consisting of a screenplay for a video, based on a source work."@en, "Expression d’une œuvre consistant en le scénario pour une vidéo, basée sur l’œuvre source."@fr, "Una expresión de una obra que consiste en el guión para un video, basado en la obra fuente."@es ;
    rdakit:toolkitLabel "adaptada como guión para video (expresión)"@es, "adapted as video screenplay (expression)"@en, "adapté en scénario de vidéo (expression)"@fr ;
    reg:hasSubproperty <http://rdaregistry.info/Elements/e/object/P20098> ;
    reg:hasUnconstrained <http://rdaregistry.info/Elements/u/P60187> ;
    reg:lexicalAlias <http://rdaregistry.info/Elements/e/adaptedAsVideoScreenplayExpression.en> ;
    reg:name "adaptedAsVideoScreenplayExpression"@en ;
    reg:status <http://metadataregistry.org/uri/RegStatus/1001> ;
    a rdf:Property ;
    rdfs:domain <http://rdaregistry.info/Elements/c/C10006> ;
    rdfs:isDefinedBy <http://rdaregistry.info/Elements/e/> ;
    rdfs:label "is adapted as video screenplay (expression)"@en ;
    rdfs:subPropertyOf <http://rdaregistry.info/Elements/e/P20096> ;
    skos:definition "Relates an expression to an expression of a work consisting of a screenplay for a video, based on a source work."@en .

<http://rdaregistry.info/Elements/e/P20099>
    rdakit:instructionNumber "24.5" ;
    rdakit:toolkitDefinition "An expression of a work consisting of a script for a radio program, based on a source work."@en, "Expression d’une œuvre consistant en le script d’une émission de radio, basée sur l’œuvre source."@fr, "Una expresión de una obra que consiste en el guión de un programa de radio, basado en la obra fuente."@es ;
    rdakit:toolkitLabel "adaptada como guión radiofónico (expresión)"@es, "adapted as radio script (expression)"@en, "adapté en script radiophonique (expression)"@fr ;
    reg:hasSubproperty <http://rdaregistry.info/Elements/e/object/P20099> ;
    reg:hasUnconstrained <http://rdaregistry.info/Elements/u/P60188> ;
    reg:lexicalAlias <http://rdaregistry.info/Elements/e/adaptedAsRadioScriptExpression.en> ;
    reg:name "adaptedAsRadioScriptExpression"@en ;
    reg:status <http://metadataregistry.org/uri/RegStatus/1001> ;
    a rdf:Property ;
    rdfs:domain <http://rdaregistry.info/Elements/c/C10006> ;
    rdfs:isDefinedBy <http://rdaregistry.info/Elements/e/> ;
    rdfs:label "is adapted as radio script (expression)"@en ;
    rdfs:subPropertyOf <http://rdaregistry.info/Elements/e/P20153> ;
    skos:definition "Relates an expression to an expression of a work consisting of a script for a radio program, based on a source work."@en .

<http://rdaregistry.info/Elements/e/P20100>
    rdakit:instructionNumber "24.5" ;
    rdakit:toolkitDefinition "An expression of a work paired with another expression without either expression being considered to predominate."@en, "Expression d’une œuvre appariée à une autre expression sans qu’aucune des deux expressions ne soit considérée comme prédominante."@fr, "Una expresión de una obra unida con otra entidad sin que ninguna pueda ser considerada como principal"@es ;
    rdakit:toolkitLabel "complementada por (expresión)"@es, "complemented by (expression)"@en, "complété par (expression)"@fr ;
    reg:hasSubproperty <http://rdaregistry.info/Elements/e/P20084>, <http://rdaregistry.info/Elements/e/P20102>, <http://rdaregistry.info/Elements/e/P20157>, <http://rdaregistry.info/Elements/e/P20160>, <http://rdaregistry.info/Elements/e/P20163>, <http://rdaregistry.info/Elements/e/P20176>, <http://rdaregistry.info/Elements/e/P20253>, <http://rdaregistry.info/Elements/e/P20254>, <http://rdaregistry.info/Elements/e/object/P20100> ;
    reg:hasUnconstrained <http://rdaregistry.info/Elements/u/P60198> ;
    reg:lexicalAlias <http://rdaregistry.info/Elements/e/complementedByExpression.en> ;
    reg:name "complementedByExpression"@en ;
    reg:status <http://metadataregistry.org/uri/RegStatus/1001> ;
    a rdf:Property ;
    rdfs:domain <http://rdaregistry.info/Elements/c/C10006> ;
    rdfs:isDefinedBy <http://rdaregistry.info/Elements/e/> ;
    rdfs:label "is complemented by (expression)"@en ;
    rdfs:subPropertyOf <http://rdaregistry.info/Elements/e/P20232> ;
    skos:definition "Relates an expression to an expression of a work paired with another expression without either expression being considered to predominate."@en .

<http://rdaregistry.info/Elements/e/P20101>
    rdakit:instructionNumber "24.5" ;
    rdakit:toolkitDefinition "An expression of a work part of whose content separated from an earlier expression to form a new expression."@en, "Expression d’une œuvre dont une partie du contenu a été détachée d’une expression antérieure pour former une nouvelle expression."@fr, "Una expresión de una obra parte de cuyo contenido se separó de una expresión anterior para formar una nueva expresión."@es ;
    rdakit:toolkitLabel "continuada en parte por (expresión)"@es, "continued in part by (expression)"@en, "continué en partie par (expression)"@fr ;
    reg:hasSubproperty <http://rdaregistry.info/Elements/e/object/P20101> ;
    reg:hasUnconstrained <http://rdaregistry.info/Elements/u/P60199> ;
    reg:lexicalAlias <http://rdaregistry.info/Elements/e/continuedInPartByExpression.en> ;
    reg:name "continuedInPartByExpression"@en ;
    reg:status <http://metadataregistry.org/uri/RegStatus/1001> ;
    a rdf:Property ;
    rdfs:domain <http://rdaregistry.info/Elements/c/C10006> ;
    rdfs:isDefinedBy <http://rdaregistry.info/Elements/e/> ;
    rdfs:label "is continued in part by (expression)"@en ;
    rdfs:subPropertyOf <http://rdaregistry.info/Elements/e/P20169> ;
    skos:definition "Relates an expression to an expression of a work part of whose content separated from an earlier expression to form a new expression."@en ;
    skos:scopeNote "This relationship applies generally to serials."@en .

<http://rdaregistry.info/Elements/e/P20102>
    rdakit:instructionNumber "24.5" ;
    rdakit:toolkitDefinition "An expression of a work such as a motion picture, television program, or video, that uses the text of a work as a screenplay."@en, "Expression d’une œuvre telle qu’un film, une émission de télévision ou une vidéo qui utilise le texte de l’œuvre comme scénario."@fr, "Una expresión de una obra tal como una película cinematográfica, programa de televisión o video, que utiliza el texto de la obra como un guión cinematográfico."@es ;
    rdakit:toolkitLabel "guión para (expresión)"@es, "screenplay for (expression)"@en, "scénario pour (expression)"@fr ;
    reg:hasSubproperty <http://rdaregistry.info/Elements/e/P20173>, <http://rdaregistry.info/Elements/e/P20174>, <http://rdaregistry.info/Elements/e/P20175>, <http://rdaregistry.info/Elements/e/object/P20102> ;
    reg:hasUnconstrained <http://rdaregistry.info/Elements/u/P60201> ;
    reg:lexicalAlias <http://rdaregistry.info/Elements/e/screenplayForExpression.en> ;
    reg:name "screenplayForExpression"@en ;
    reg:status <http://metadataregistry.org/uri/RegStatus/1001> ;
    a rdf:Property ;
    rdfs:domain <http://rdaregistry.info/Elements/c/C10006> ;
    rdfs:isDefinedBy <http://rdaregistry.info/Elements/e/> ;
    rdfs:label "is screenplay for (expression)"@en ;
    rdfs:subPropertyOf <http://rdaregistry.info/Elements/e/P20100> ;
    skos:definition "Relates an expression to an expression of a work such as a motion picture, television program, or video, that uses the text of a work as a screenplay."@en .

<http://rdaregistry.info/Elements/e/P20103>
    rdakit:instructionNumber "24.5" ;
    rdakit:toolkitDefinition "An expression of a work such as a play or other spoken work for the stage that uses a musical work as incidental music."@en, "Expression d’une œuvre telle qu’une pièce de théâtre ou une autre œuvre parlée pour la scène qui utilise l’œuvre musicale comme musique de scène."@fr, "Una expresión de una obra tal como una obra de teatro u otra obra hablada para escena que usa la obra musical como música incidental."@es ;
    rdakit:toolkitLabel "incidental music for (expression)"@en, "musique de scène pour (expression)"@fr, "música incidental de (expresión)"@es ;
    reg:hasSubproperty <http://rdaregistry.info/Elements/e/object/P20103> ;
    reg:hasUnconstrained <http://rdaregistry.info/Elements/u/P60202> ;
    reg:lexicalAlias <http://rdaregistry.info/Elements/e/incidentalMusicForExpression.en> ;
    reg:name "incidentalMusicForExpression"@en ;
    reg:status <http://metadataregistry.org/uri/RegStatus/1001> ;
    a rdf:Property ;
    rdfs:domain <http://rdaregistry.info/Elements/c/C10006> ;
    rdfs:isDefinedBy <http://rdaregistry.info/Elements/e/> ;
    rdfs:label "is incidental music for (expression)"@en ;
    rdfs:subPropertyOf <http://rdaregistry.info/Elements/e/P20244> ;
    skos:definition "Relates an expression to an expression of a work such as a play or other spoken work for the stage that uses a musical work as incidental music."@en .

<http://rdaregistry.info/Elements/e/P20104>
    rdakit:instructionNumber "24.5" ;
    rdakit:toolkitDefinition "An expression of a work that abbreviates a source expression in a brief, objective manner."@en, "Expression d’une œuvre qui abrège l’expression source d’une manière brève et objective."@fr, "Una expresión de una obra que abrevia la expresión fuente en una forma breve y objetiva."@es ;
    rdakit:toolkitLabel "abstracted as (expression)"@en, "resumida como (expresión)"@es, "résumé analytiquement comme (expression)"@fr ;
    reg:hasSubproperty <http://rdaregistry.info/Elements/e/object/P20104> ;
    reg:hasUnconstrained <http://rdaregistry.info/Elements/u/P60203> ;
    reg:lexicalAlias <http://rdaregistry.info/Elements/e/abstractedAsExpression.en> ;
    reg:name "abstractedAsExpression"@en ;
    reg:status <http://metadataregistry.org/uri/RegStatus/1001> ;
    a rdf:Property ;
    rdfs:domain <http://rdaregistry.info/Elements/c/C10006> ;
    rdfs:isDefinedBy <http://rdaregistry.info/Elements/e/> ;
    rdfs:label "is abstracted as (expression)"@en ;
    rdfs:subPropertyOf <http://rdaregistry.info/Elements/e/P20203> ;
    skos:definition "Relates an expression to an expression of a work that abbreviates a source expression in a brief, objective manner."@en .

<http://rdaregistry.info/Elements/e/P20105>
    rdakit:instructionNumber "24.5" ;
    rdakit:toolkitDefinition "An expression of a work that adds to the content of a predominant expression."@en, "Expression d’une œuvre qui ajoute au contenu d’une expression prédominante."@fr, "Una expresión de una obra que añade al contenido de una expresión principal."@es ;
    rdakit:toolkitLabel "augmented by (expression)"@en, "augmenté par (expression)"@fr, "aumentada por (expresión)"@es ;
    reg:hasSubproperty <http://rdaregistry.info/Elements/e/P20080>, <http://rdaregistry.info/Elements/e/P20093>, <http://rdaregistry.info/Elements/e/P20094>, <http://rdaregistry.info/Elements/e/P20107>, <http://rdaregistry.info/Elements/e/P20108>, <http://rdaregistry.info/Elements/e/P20109>, <http://rdaregistry.info/Elements/e/P20118>, <http://rdaregistry.info/Elements/e/P20120>, <http://rdaregistry.info/Elements/e/P20155>, <http://rdaregistry.info/Elements/e/P20156>, <http://rdaregistry.info/Elements/e/P20172>, <http://rdaregistry.info/Elements/e/object/P20105> ;
    reg:hasUnconstrained <http://rdaregistry.info/Elements/u/P60204> ;
    reg:lexicalAlias <http://rdaregistry.info/Elements/e/augmentedByExpression.en> ;
    reg:name "augmentedByExpression"@en ;
    reg:status <http://metadataregistry.org/uri/RegStatus/1001> ;
    a rdf:Property ;
    rdfs:domain <http://rdaregistry.info/Elements/c/C10006> ;
    rdfs:isDefinedBy <http://rdaregistry.info/Elements/e/> ;
    rdfs:label "is augmented by (expression)"@en ;
    rdfs:subPropertyOf <http://rdaregistry.info/Elements/e/P20232> ;
    skos:definition "Relates an expression to an expression of a work that adds to the content of a predominant expression."@en .

<http://rdaregistry.info/Elements/e/P20106>
    rdakit:instructionNumber "24.5" ;
    rdakit:toolkitDefinition "An expression of a work that consists of a brief recapitulation of the content of a source expression."@en, "Expression d’une œuvre qui consiste en une brève récapitulation du contenu de l’expression source."@fr, "Una expresión de una obra que consiste en una recapitulación breve del contenido de la expresión fuente."@es ;
    rdakit:toolkitLabel "résumé comme (expression)"@fr, "sumarizada como (expresión)"@es, "summarized as (expression)"@en ;
    reg:hasSubproperty <http://rdaregistry.info/Elements/e/object/P20106> ;
    reg:hasUnconstrained <http://rdaregistry.info/Elements/u/P60205> ;
    reg:lexicalAlias <http://rdaregistry.info/Elements/e/summarizedAsExpression.en> ;
    reg:name "summarizedAsExpression"@en ;
    reg:status <http://metadataregistry.org/uri/RegStatus/1001> ;
    a rdf:Property ;
    rdfs:domain <http://rdaregistry.info/Elements/c/C10006> ;
    rdfs:isDefinedBy <http://rdaregistry.info/Elements/e/> ;
    rdfs:label "is summarized as (expression)"@en ;
    rdfs:subPropertyOf <http://rdaregistry.info/Elements/e/P20203> ;
    skos:definition "Relates an expression to an expression of a work that consists of a brief recapitulation of the content of a source expression."@en .

<http://rdaregistry.info/Elements/e/P20107>
    rdakit:instructionNumber "24.5" ;
    rdakit:toolkitDefinition "An expression of a work that consists of a complete enumeration of items arranged systematically."@en, "Expression d’une œuvre qui consiste en une énumération complète des items classés systématiquement."@fr, "Una expresión de una obra que consiste en una enumeración completa de ítems ordenados sistemáticamente."@es ;
    rdakit:toolkitLabel "catalogue (expression)"@en, "catalogue (expression)"@fr, "catálogo (expresión)"@es ;
    reg:hasSubproperty <http://rdaregistry.info/Elements/e/object/P20107> ;
    reg:hasUnconstrained <http://rdaregistry.info/Elements/u/P60206> ;
    reg:lexicalAlias <http://rdaregistry.info/Elements/e/catalogueExpression.en> ;
    reg:name "catalogueExpression"@en ;
    reg:status <http://metadataregistry.org/uri/RegStatus/1001> ;
    a rdf:Property ;
    rdfs:domain <http://rdaregistry.info/Elements/c/C10006> ;
    rdfs:isDefinedBy <http://rdaregistry.info/Elements/e/> ;
    rdfs:label "is catalogue (expression)"@en ;
    rdfs:subPropertyOf <http://rdaregistry.info/Elements/e/P20105> ;
    skos:definition "Relates an expression to an expression of a work that consists of a complete enumeration of items arranged systematically."@en .

<http://rdaregistry.info/Elements/e/P20108>
    rdakit:instructionNumber "24.5" ;
    rdakit:toolkitDefinition "An expression of a work that consists of an index of all the words in a predominant expression."@en, "Expression d’une œuvre qui consiste en un index de tous les mots de l’expression prédominante."@fr, "Una expresión de una obra que consiste en un índice de todas las palabras en la expresión principal."@es ;
    rdakit:toolkitLabel "concordance (expression)"@en, "concordance (expression)"@fr, "concordancia (expresión)"@es ;
    reg:hasSubproperty <http://rdaregistry.info/Elements/e/object/P20108> ;
    reg:hasUnconstrained <http://rdaregistry.info/Elements/u/P60208> ;
    reg:lexicalAlias <http://rdaregistry.info/Elements/e/concordanceExpression.en> ;
    reg:name "concordanceExpression"@en ;
    reg:status <http://metadataregistry.org/uri/RegStatus/1001> ;
    a rdf:Property ;
    rdfs:domain <http://rdaregistry.info/Elements/c/C10006> ;
    rdfs:isDefinedBy <http://rdaregistry.info/Elements/e/> ;
    rdfs:label "is concordance (expression)"@en ;
    rdfs:subPropertyOf <http://rdaregistry.info/Elements/e/P20105> ;
    skos:definition "Relates an expression to an expression of a work that consists of an index of all the words in a predominant expression."@en .

<http://rdaregistry.info/Elements/e/P20109>
    rdakit:instructionNumber "24.5" ;
    rdakit:toolkitDefinition "An expression of a work consisting of brief content that is essential for the completeness of an expression of another work."@en, "Expression d’une œuvre qui consiste en brèves informations additionnelles, moins étendues qu’un supplément, mais essentielles à la complétude du texte de l’œuvre prédominante ; ces informations sont généralement ajoutées à la fin du contenu, mais peuvent aussi parfois être publiées séparément."@fr, "Una expresión de una obra que consiste en material adicional breve, menos extenso que un suplemento, pero esencial para la integridad del texto de la obra principal; generalmente se añade al final del contenido, pero algunas veces se publica separadamente."@es ;
    rdakit:toolkitLabel "addenda (expression)"@en, "addenda (expression)"@fr, "adenda (expresión)"@es ;
    reg:hasSubproperty <http://rdaregistry.info/Elements/e/object/P20109> ;
    reg:hasUnconstrained <http://rdaregistry.info/Elements/u/P60209> ;
    reg:lexicalAlias <http://rdaregistry.info/Elements/e/addendaExpression.en> ;
    reg:name "addendaExpression"@en ;
    reg:status <http://metadataregistry.org/uri/RegStatus/1001> ;
    a rdf:Property ;
    rdfs:domain <http://rdaregistry.info/Elements/c/C10006> ;
    rdfs:isDefinedBy <http://rdaregistry.info/Elements/e/> ;
    rdfs:label "is addenda (expression)"@en ;
    rdfs:subPropertyOf <http://rdaregistry.info/Elements/e/P20105> ;
    skos:definition "Relates an expression to an expression of a work consisting of brief content that is essential for the completeness of an expression of another work."@en .

<http://rdaregistry.info/Elements/e/P20110>
    rdakit:instructionNumber "24.5" ;
    rdakit:toolkitDefinition "An expression of a work consisting of the text of an opera or other work for the musical stage, or an oratorio, based on a source work."@en, "Expression d’une œuvre qui consiste en le texte d’un opéra ou d’une autre œuvre pour la scène musicale, ou bien d’un oratorio, basée sur l’œuvre source."@fr, "Una expresión de una obra que consiste en el texto de una ópera u otra obra para representación musical, u oratorio, basada en la obra fuente."@es ;
    rdakit:toolkitLabel "adaptada como libreto (expresión)"@es, "adapted as libretto (expression)"@en, "adapté en livret (expression)"@fr ;
    reg:hasSubproperty <http://rdaregistry.info/Elements/e/object/P20110> ;
    reg:hasUnconstrained <http://rdaregistry.info/Elements/u/P60210> ;
    reg:lexicalAlias <http://rdaregistry.info/Elements/e/adaptedAsLibrettoExpression.en> ;
    reg:name "adaptedAsLibrettoExpression"@en ;
    reg:status <http://metadataregistry.org/uri/RegStatus/1001> ;
    a rdf:Property ;
    rdfs:domain <http://rdaregistry.info/Elements/c/C10006> ;
    rdfs:isDefinedBy <http://rdaregistry.info/Elements/e/> ;
    rdfs:label "is adapted as libretto (expression)"@en ;
    rdfs:subPropertyOf <http://rdaregistry.info/Elements/e/P20153> ;
    skos:definition "Relates an expression to an expression of a work consisting of the text of an opera or other work for the musical stage, or an oratorio, based on a source work."@en .

<http://rdaregistry.info/Elements/e/P20111>
    reg:status <http://metadataregistry.org/uri/RegStatus/1008> ;
    a rdf:Property ;
    rdfs:isDefinedBy <http://rdaregistry.info/Elements/e/> ;
    rdfs:subPropertyOf <http://rdaregistry.info/Elements/e/P20202> .

<http://rdaregistry.info/Elements/e/P20112>
    reg:status <http://metadataregistry.org/uri/RegStatus/1008> ;
    a rdf:Property ;
    rdfs:isDefinedBy <http://rdaregistry.info/Elements/e/> ;
    rdfs:subPropertyOf <http://rdaregistry.info/Elements/e/P20202> .

<http://rdaregistry.info/Elements/e/P20113>
    reg:status <http://metadataregistry.org/uri/RegStatus/1008> ;
    a rdf:Property ;
    rdfs:isDefinedBy <http://rdaregistry.info/Elements/e/> ;
    rdfs:subPropertyOf <http://rdaregistry.info/Elements/e/P20202> .

<http://rdaregistry.info/Elements/e/P20114>
    rdakit:instructionNumber "24.5" ;
    rdakit:toolkitDefinition "An expression of a work that copies the style or content of the source work."@en, "Expression d’une œuvre qui copie le style ou le contenu de l’œuvre source."@fr, "Una expresión de una obra que copia el estilo o contenido de la obra fuente."@es ;
    rdakit:toolkitLabel "imitada como (expresión)"@es, "imitated as (expression)"@en, "imité comme (expression)"@fr ;
    reg:hasSubproperty <http://rdaregistry.info/Elements/e/P20142>, <http://rdaregistry.info/Elements/e/object/P20114> ;
    reg:hasUnconstrained <http://rdaregistry.info/Elements/u/P60214> ;
    reg:lexicalAlias <http://rdaregistry.info/Elements/e/imitatedAsExpression.en> ;
    reg:name "imitatedAsExpression"@en ;
    reg:status <http://metadataregistry.org/uri/RegStatus/1001> ;
    a rdf:Property ;
    rdfs:domain <http://rdaregistry.info/Elements/c/C10006> ;
    rdfs:isDefinedBy <http://rdaregistry.info/Elements/e/> ;
    rdfs:label "is imitated as (expression)"@en ;
    rdfs:subPropertyOf <http://rdaregistry.info/Elements/e/P20203> ;
    skos:definition "Relates an expression to an expression of a work that copies the style or content of a source work."@en .

<http://rdaregistry.info/Elements/e/P20115>
    rdakit:instructionNumber "24.5" ;
    rdakit:toolkitDefinition "An expression of a work that enlarges upon the content of the source work."@en, "Expression d’une œuvre qui accroît le contenu de l’œuvre source."@fr, "Una expresión de una obra que extiende el contenido de la obra fuente."@es ;
    rdakit:toolkitLabel "ampliada como (expresión)"@es, "augmenté comme (expression)"@fr, "expanded as (expression)"@en ;
    reg:hasSubproperty <http://rdaregistry.info/Elements/e/object/P20115> ;
    reg:hasUnconstrained <http://rdaregistry.info/Elements/u/P60216> ;
    reg:lexicalAlias <http://rdaregistry.info/Elements/e/expandedAsExpression.en> ;
    reg:name "expandedAsExpression"@en ;
    reg:status <http://metadataregistry.org/uri/RegStatus/1001> ;
    a rdf:Property ;
    rdfs:domain <http://rdaregistry.info/Elements/c/C10006> ;
    rdfs:isDefinedBy <http://rdaregistry.info/Elements/e/> ;
    rdfs:label "is expanded as (expression)"@en ;
    rdfs:subPropertyOf <http://rdaregistry.info/Elements/e/P20203> ;
    skos:definition "Relates an expression to an expression of a work that enlarges upon the content of a source work."@en .

<http://rdaregistry.info/Elements/e/P20116>
    reg:status <http://metadataregistry.org/uri/RegStatus/1008> ;
    a rdf:Property ;
    rdfs:isDefinedBy <http://rdaregistry.info/Elements/e/> ;
    rdfs:subPropertyOf <http://rdaregistry.info/Elements/e/P20202> .

<http://rdaregistry.info/Elements/e/P20117>
    reg:status <http://metadataregistry.org/uri/RegStatus/1008> ;
    a rdf:Property ;
    rdfs:isDefinedBy <http://rdaregistry.info/Elements/e/> ;
    rdfs:subPropertyOf <http://rdaregistry.info/Elements/e/P20202> .

<http://rdaregistry.info/Elements/e/P20118>
    rdakit:instructionNumber "24.5" ;
    rdakit:toolkitDefinition "An expression of a work whose content augments an expression of another work."@en, "Expression d’une œuvre qui forme une partie augmentante d’une autre œuvre et qui n’est pas essentielle à la complétude du contenu, telle qu’une liste de références, des tableaux statistiques et des indications explicatives ; elle peut soit figurer à la fin du contenu de l’œuvre prédominante, soit être publiée séparément."@fr, "Una expresión de una obra que forma una parte adicional de otra obra y que no es esencial para la integridad del contenido, tal como una lista de referencias, tablas estadísticas y material explicativo; puede ser material que se presenta al final del contenido de la obra principal, o ser publicado separadamente."@es ;
    rdakit:toolkitLabel "annexe (expression)"@fr, "appendix (expression)"@en, "apéndice (expresión)"@es ;
    reg:hasSubproperty <http://rdaregistry.info/Elements/e/object/P20118> ;
    reg:hasUnconstrained <http://rdaregistry.info/Elements/u/P60221> ;
    reg:lexicalAlias <http://rdaregistry.info/Elements/e/appendixExpression.en> ;
    reg:name "appendixExpression"@en ;
    reg:status <http://metadataregistry.org/uri/RegStatus/1001> ;
    a rdf:Property ;
    rdfs:domain <http://rdaregistry.info/Elements/c/C10006> ;
    rdfs:isDefinedBy <http://rdaregistry.info/Elements/e/> ;
    rdfs:label "is appendix (expression)"@en ;
    rdfs:subPropertyOf <http://rdaregistry.info/Elements/e/P20105> ;
    skos:definition "Relates an expression to an expression of a work whose content augments an expression of another work."@en ;
    skos:scopeNote "Includes lists of references, statistical tables, and explanatory matter that are not essential to the completeness of the content."@en .

<http://rdaregistry.info/Elements/e/P20119>
    rdakit:instructionNumber "24.5" ;
    rdakit:toolkitDefinition "An expression of a work that is both an adaptation and a translation into another language of a source expression."@en, "Expression d’une œuvre qui traduit librement le texte dans une autre langue, de façon à préserver l’esprit de l’original, mais non ses particularités linguistiques."@fr, "Una expresión de una obra que traduce libremente el texto en otra lengua, preservando el espíritu del original, pero no sus detalles lingüísticos."@es ;
    rdakit:toolkitLabel "freely translated as (expression)"@en, "librement traduit comme (expression)"@fr, "traducida libremente como (expresión)"@es ;
    reg:hasSubproperty <http://rdaregistry.info/Elements/e/object/P20119> ;
    reg:hasUnconstrained <http://rdaregistry.info/Elements/u/P60189> ;
    reg:lexicalAlias <http://rdaregistry.info/Elements/e/freelyTranslatedAsExpression.en> ;
    reg:name "freelyTranslatedAsExpression"@en ;
    reg:status <http://metadataregistry.org/uri/RegStatus/1001> ;
    a rdf:Property ;
    rdfs:domain <http://rdaregistry.info/Elements/c/C10006> ;
    rdfs:isDefinedBy <http://rdaregistry.info/Elements/e/> ;
    rdfs:label "is freely translated as (expression)"@en ;
    rdfs:subPropertyOf <http://rdaregistry.info/Elements/e/P20203> ;
    skos:definition "Relates an expression to an expression of a work that is both an adaptation and a translation into another language of a source expression."@en .

<http://rdaregistry.info/Elements/e/P20120>
    rdakit:instructionNumber "24.5" ;
    rdakit:toolkitDefinition "An expression of a work that guides a user through the use of a predominant work, using notes, learning and study aids, exercises, problems, questions and answers, instructor or student materials, etc."@en, "Expression d’une œuvre qui guide un utilisateur à travers l’œuvre prédominante au moyen de notes, d’outils pédagogiques, d’exercices, de problèmes, de questions et réponses, de matériel didactique, etc."@fr, "Una expresión de una obra que guía al usuario a través del uso de la obra principal, utilizando notas, ayudas de aprendizaje y estudio, ejercicios, problemas, preguntas y respuestas, materiales para el instructor o el estudiante, etc."@es ;
    rdakit:toolkitLabel "guide (expression)"@en, "guide (expression)"@fr, "guía (expresión)"@es ;
    reg:hasSubproperty <http://rdaregistry.info/Elements/e/object/P20120> ;
    reg:hasUnconstrained <http://rdaregistry.info/Elements/u/P60222> ;
    reg:lexicalAlias <http://rdaregistry.info/Elements/e/guideExpression.en> ;
    reg:name "guideExpression"@en ;
    reg:status <http://metadataregistry.org/uri/RegStatus/1001> ;
    a rdf:Property ;
    rdfs:domain <http://rdaregistry.info/Elements/c/C10006> ;
    rdfs:isDefinedBy <http://rdaregistry.info/Elements/e/> ;
    rdfs:label "is guide (expression)"@en ;
    rdfs:subPropertyOf <http://rdaregistry.info/Elements/e/P20105> ;
    skos:definition "Relates an expression to an expression of a work that guides a user through the use of a predominant work, using notes, learning and study aids, exercises, problems, questions and answers, instructor or student materials, etc."@en .

<http://rdaregistry.info/Elements/e/P20121>
    rdakit:instructionNumber "24.5" ;
    rdakit:toolkitDefinition "An expression of a work that has been abridged, i.e., shortened without changing the general meaning or manner of presentation of a source work."@en, "Expression d’une œuvre qui a été abrégée, c’est-à-dire raccourcie sans changer le sens général ou le mode de présentation de l’œuvre source."@fr, "Una expresión de una obra que fue abreviada, i.e., acortada sin cambiar el sentido general o la manera de presentación de la obra fuente."@es ;
    rdakit:toolkitLabel "abreviada de (expresión)"@es, "abridgement of (expression)"@en, "abrégé de (expression)"@fr ;
    reg:hasSubproperty <http://rdaregistry.info/Elements/e/object/P20121> ;
    reg:hasUnconstrained <http://rdaregistry.info/Elements/u/P60223> ;
    reg:lexicalAlias <http://rdaregistry.info/Elements/e/abridgementOfExpression.en> ;
    reg:name "abridgementOfExpression"@en ;
    reg:status <http://metadataregistry.org/uri/RegStatus/1001> ;
    a rdf:Property ;
    rdfs:domain <http://rdaregistry.info/Elements/c/C10006> ;
    rdfs:isDefinedBy <http://rdaregistry.info/Elements/e/> ;
    rdfs:label "is abridgement of (expression)"@en ;
    rdfs:subPropertyOf <http://rdaregistry.info/Elements/e/P20204> ;
    skos:definition "Relates an expression to an expression of a work that has been abridged, i.e., shortened without changing the general meaning or manner of presentation of a source work."@en .

<http://rdaregistry.info/Elements/e/P20122>
    rdakit:instructionNumber "24.5" ;
    rdakit:toolkitDefinition "An expression of a work that has been abstracted, i.e., abbreviated in a brief, objective manner."@en, "Expression d’une œuvre qui a été résumée analytiquement, c’est-à-dire abrégée d’une manière brève et objective."@fr, "Una expresión de una obra que fue resumida, i.e., abreviada en una forma breve, objetiva."@es ;
    rdakit:toolkitLabel "abstract of (expression)"@en, "resumen de (expresión)"@es, "résumé analytique de (expression)"@fr ;
    reg:hasSubproperty <http://rdaregistry.info/Elements/e/object/P20122> ;
    reg:hasUnconstrained <http://rdaregistry.info/Elements/u/P60224> ;
    reg:lexicalAlias <http://rdaregistry.info/Elements/e/abstractOfExpression.en> ;
    reg:name "abstractOfExpression"@en ;
    reg:status <http://metadataregistry.org/uri/RegStatus/1001> ;
    a rdf:Property ;
    rdfs:domain <http://rdaregistry.info/Elements/c/C10006> ;
    rdfs:isDefinedBy <http://rdaregistry.info/Elements/e/> ;
    rdfs:label "is abstract of (expression)"@en ;
    rdfs:subPropertyOf <http://rdaregistry.info/Elements/e/P20204> ;
    skos:definition "Relates an expression to an expression of a work that has been abstracted, i.e., abbreviated in a brief, objective manner."@en .

<http://rdaregistry.info/Elements/e/P20123>
    rdakit:instructionNumber "24.5" ;
    rdakit:toolkitDefinition "An expression of a work that has been adapted as a drama."@en, "Expression d’une œuvre qui a été adaptée en pièce de théâtre."@fr, "Una expresión de una obra que fue adaptada como drama."@es ;
    rdakit:toolkitLabel "adaptation au théâtre de (expression)"@fr, "dramatización de (expresión)"@es, "dramatization of (expression)"@en ;
    reg:hasSubproperty <http://rdaregistry.info/Elements/e/object/P20123> ;
    reg:hasUnconstrained <http://rdaregistry.info/Elements/u/P60225> ;
    reg:lexicalAlias <http://rdaregistry.info/Elements/e/dramatizationOfExpression.en> ;
    reg:name "dramatizationOfExpression"@en ;
    reg:status <http://metadataregistry.org/uri/RegStatus/1001> ;
    a rdf:Property ;
    rdfs:domain <http://rdaregistry.info/Elements/c/C10006> ;
    rdfs:isDefinedBy <http://rdaregistry.info/Elements/e/> ;
    rdfs:label "is dramatization of (expression)"@en ;
    rdfs:subPropertyOf <http://rdaregistry.info/Elements/e/P20152> ;
    skos:definition "Relates an expression to an expression of a work that has been adapted as a drama."@en .

<http://rdaregistry.info/Elements/e/P20124>
    rdakit:instructionNumber "24.5" ;
    rdakit:toolkitDefinition "An expression of a work that has been adapted as a literary composition in verse form."@en, "Expression d’une œuvre qui a été adaptée sous forme de composition littéraire en vers."@fr, "Una expresión de una obra que fue adaptada como una composición literaria en forma de verso."@es ;
    rdakit:toolkitLabel "adaptación en verso de (expresión)"@es, "adaptation en vers de (expression)"@fr, "verse adaptation of (expression)"@en ;
    reg:hasSubproperty <http://rdaregistry.info/Elements/e/object/P20124> ;
    reg:hasUnconstrained <http://rdaregistry.info/Elements/u/P60226> ;
    reg:lexicalAlias <http://rdaregistry.info/Elements/e/verseAdaptationOfExpression.en> ;
    reg:name "verseAdaptationOfExpression"@en ;
    reg:status <http://metadataregistry.org/uri/RegStatus/1001> ;
    a rdf:Property ;
    rdfs:domain <http://rdaregistry.info/Elements/c/C10006> ;
    rdfs:isDefinedBy <http://rdaregistry.info/Elements/e/> ;
    rdfs:label "is verse adaptation of (expression)"@en ;
    rdfs:subPropertyOf <http://rdaregistry.info/Elements/e/P20152> ;
    skos:definition "Relates an expression to an expression of a work that has been adapted as a literary composition in verse form."@en .

<http://rdaregistry.info/Elements/e/P20125>
    rdakit:instructionNumber "24.5" ;
    rdakit:toolkitDefinition "An expression of a work that has been adapted as a motion picture."@en, "Expression d’une œuvre qui a été adaptée en film."@fr, "Una expresión de una obra que fue adaptada como película cinematográfica."@es ;
    rdakit:toolkitLabel "adaptación cinematográfica de (expresión)"@es, "adaptation au cinéma de (expression)"@fr, "motion picture adaptation of (expression)"@en ;
    reg:hasSubproperty <http://rdaregistry.info/Elements/e/object/P20125> ;
    reg:hasUnconstrained <http://rdaregistry.info/Elements/u/P60227> ;
    reg:lexicalAlias <http://rdaregistry.info/Elements/e/motionPictureAdaptationOfExpression.en> ;
    reg:name "motionPictureAdaptationOfExpression"@en ;
    reg:status <http://metadataregistry.org/uri/RegStatus/1001> ;
    a rdf:Property ;
    rdfs:domain <http://rdaregistry.info/Elements/c/C10006> ;
    rdfs:isDefinedBy <http://rdaregistry.info/Elements/e/> ;
    rdfs:label "is motion picture adaptation of (expression)"@en ;
    rdfs:subPropertyOf <http://rdaregistry.info/Elements/e/P20152> ;
    skos:definition "Relates an expression to an expression of a work that has been adapted as a motion picture."@en .

<http://rdaregistry.info/Elements/e/P20126>
    rdakit:instructionNumber "24.5" ;
    rdakit:toolkitDefinition "An expression of a work that has been adapted as a novel."@en, "Expression d’une œuvre qui a été adaptée en roman."@fr, "Una expresión de una obra que fue adaptada como novela."@es ;
    rdakit:toolkitLabel "novelización de (expresión)"@es, "novelization of (expression)"@en, "novélisation de (expression)"@fr ;
    reg:hasSubproperty <http://rdaregistry.info/Elements/e/object/P20126> ;
    reg:hasUnconstrained <http://rdaregistry.info/Elements/u/P60228> ;
    reg:lexicalAlias <http://rdaregistry.info/Elements/e/novelizationOfExpression.en> ;
    reg:name "novelizationOfExpression"@en ;
    reg:status <http://metadataregistry.org/uri/RegStatus/1001> ;
    a rdf:Property ;
    rdfs:domain <http://rdaregistry.info/Elements/c/C10006> ;
    rdfs:isDefinedBy <http://rdaregistry.info/Elements/e/> ;
    rdfs:label "is novelization of (expression)"@en ;
    rdfs:subPropertyOf <http://rdaregistry.info/Elements/e/P20152> ;
    skos:definition "Relates an expression to an expression of a work that has been adapted as a novel."@en .

<http://rdaregistry.info/Elements/e/P20127>
    rdakit:instructionNumber "24.5" ;
    rdakit:toolkitDefinition "An expression of a work that has been adapted as a radio program."@en, "Expression d’une œuvre qui a été adaptée en émission de radio."@fr, "Una expresión de una obra que fue adaptada como programa de radio."@es ;
    rdakit:toolkitLabel "adaptación para radio de (expresión)"@es, "adaptation pour la radio de (expression)"@fr, "radio adaptation of (expression)"@en ;
    reg:hasSubproperty <http://rdaregistry.info/Elements/e/object/P20127> ;
    reg:hasUnconstrained <http://rdaregistry.info/Elements/u/P60229> ;
    reg:lexicalAlias <http://rdaregistry.info/Elements/e/radioAdaptationOfExpression.en> ;
    reg:name "radioAdaptationOfExpression"@en ;
    reg:status <http://metadataregistry.org/uri/RegStatus/1001> ;
    a rdf:Property ;
    rdfs:domain <http://rdaregistry.info/Elements/c/C10006> ;
    rdfs:isDefinedBy <http://rdaregistry.info/Elements/e/> ;
    rdfs:label "is radio adaptation of (expression)"@en ;
    rdfs:subPropertyOf <http://rdaregistry.info/Elements/e/P20152> ;
    skos:definition "Relates an expression to an expression of a work that has been adapted as a radio program."@en .

<http://rdaregistry.info/Elements/e/P20128>
    rdakit:instructionNumber "24.5" ;
    rdakit:toolkitDefinition "An expression of a work that has been adapted as a television program."@en, "Expression d’une œuvre qui a été adaptée en émission de télévision."@fr, "Una expresión de una obra que fue adaptada como programa de televisión."@es ;
    rdakit:toolkitLabel "adaptación para televisión de (expresión)"@es, "adaptation pour la télévision de (expression)"@fr, "television adaptation of (expression)"@en ;
    reg:hasSubproperty <http://rdaregistry.info/Elements/e/object/P20128> ;
    reg:hasUnconstrained <http://rdaregistry.info/Elements/u/P60230> ;
    reg:lexicalAlias <http://rdaregistry.info/Elements/e/televisionAdaptationOfExpression.en> ;
    reg:name "televisionAdaptationOfExpression"@en ;
    reg:status <http://metadataregistry.org/uri/RegStatus/1001> ;
    a rdf:Property ;
    rdfs:domain <http://rdaregistry.info/Elements/c/C10006> ;
    rdfs:isDefinedBy <http://rdaregistry.info/Elements/e/> ;
    rdfs:label "is television adaptation of (expression)"@en ;
    rdfs:subPropertyOf <http://rdaregistry.info/Elements/e/P20152> ;
    skos:definition "Relates an expression to an expression of a work that has been adapted as a television program."@en .

<http://rdaregistry.info/Elements/e/P20129>
    rdakit:instructionNumber "24.5" ;
    rdakit:toolkitDefinition "An expression of a work that has been adapted as a screenplay for a motion picture, television program, or video."@en, "Expression d’une œuvre qui a été adaptée en scénario pour un film, une émission de télévision ou une vidéo."@fr, "Una expresión de una obra que fue adaptada como guión para una película cinematográfica, programa de televisión o vídeo."@es ;
    rdakit:toolkitLabel "guión basado en (expresión)"@es, "screenplay based on (expression)"@en, "scénario basé sur (expression)"@fr ;
    reg:hasSubproperty <http://rdaregistry.info/Elements/e/P20130>, <http://rdaregistry.info/Elements/e/P20131>, <http://rdaregistry.info/Elements/e/P20132>, <http://rdaregistry.info/Elements/e/object/P20129> ;
    reg:hasUnconstrained <http://rdaregistry.info/Elements/u/P60231> ;
    reg:lexicalAlias <http://rdaregistry.info/Elements/e/screenplayBasedOnExpression.en> ;
    reg:name "screenplayBasedOnExpression"@en ;
    reg:status <http://metadataregistry.org/uri/RegStatus/1001> ;
    a rdf:Property ;
    rdfs:domain <http://rdaregistry.info/Elements/c/C10006> ;
    rdfs:isDefinedBy <http://rdaregistry.info/Elements/e/> ;
    rdfs:label "is screenplay based on (expression)"@en ;
    rdfs:subPropertyOf <http://rdaregistry.info/Elements/e/P20152> ;
    skos:definition "Relates an expression to an expression of a work that has been adapted as a screenplay for a motion picture, television program, or video."@en .

<http://rdaregistry.info/Elements/e/P20130>
    rdakit:instructionNumber "24.5" ;
    rdakit:toolkitDefinition "An expression of a work that has been adapted as a screenplay for a motion picture."@en, "Expression d’une œuvre qui a été adaptée en scénario pour un film."@fr, "Una expresión de una obra que fue adaptada como guión para una película cinematográfica, programa de televisión o vídeo."@es ;
    rdakit:toolkitLabel "guión cinematográfico basado en (expresión)"@es, "motion picture screenplay based on (expression)"@en, "scénario de film basé sur (expression)"@fr ;
    reg:hasSubproperty <http://rdaregistry.info/Elements/e/object/P20130> ;
    reg:hasUnconstrained <http://rdaregistry.info/Elements/u/P60232> ;
    reg:lexicalAlias <http://rdaregistry.info/Elements/e/motionPictureScreenplayBasedOnExpression.en> ;
    reg:name "motionPictureScreenplayBasedOnExpression"@en ;
    reg:status <http://metadataregistry.org/uri/RegStatus/1001> ;
    a rdf:Property ;
    rdfs:domain <http://rdaregistry.info/Elements/c/C10006> ;
    rdfs:isDefinedBy <http://rdaregistry.info/Elements/e/> ;
    rdfs:label "is motion picture screenplay based on (expression)"@en ;
    rdfs:subPropertyOf <http://rdaregistry.info/Elements/e/P20129> ;
    skos:definition "Relates an expression to an expression of a work that has been adapted as a screenplay for a motion picture."@en .

<http://rdaregistry.info/Elements/e/P20131>
    rdakit:instructionNumber "24.5" ;
    rdakit:toolkitDefinition "An expression of a work that has been adapted as a screenplay for a television program."@en, "Expression d’une œuvre qui a été adaptée en scénario pour une émission de télévision."@fr, "Una expresión de una obra que fue adaptada como guión para un programa de televisión."@es ;
    rdakit:toolkitLabel "guión para televisión basado en (expresión)"@es, "scénario de télévision basé sur (expression)"@fr, "television screenplay based on (expression)"@en ;
    reg:hasSubproperty <http://rdaregistry.info/Elements/e/object/P20131> ;
    reg:hasUnconstrained <http://rdaregistry.info/Elements/u/P60233> ;
    reg:lexicalAlias <http://rdaregistry.info/Elements/e/televisionScreenplayBasedOnExpression.en> ;
    reg:name "televisionScreenplayBasedOnExpression"@en ;
    reg:status <http://metadataregistry.org/uri/RegStatus/1001> ;
    a rdf:Property ;
    rdfs:domain <http://rdaregistry.info/Elements/c/C10006> ;
    rdfs:isDefinedBy <http://rdaregistry.info/Elements/e/> ;
    rdfs:label "is television screenplay based on (expression)"@en ;
    rdfs:subPropertyOf <http://rdaregistry.info/Elements/e/P20129> ;
    skos:definition "Relates an expression to an expression of a work that has been adapted as a screenplay for a television program."@en .

<http://rdaregistry.info/Elements/e/P20132>
    rdakit:instructionNumber "24.5" ;
    rdakit:toolkitDefinition "An expression of a work that has been adapted as a screenplay for a video."@en, "Expression d’une œuvre qui a été adaptée en scénario pour une vidéo."@fr, "Una expresión de una obra que fue adaptada como guión para un video."@es ;
    rdakit:toolkitLabel "guión para video basado en (expresión)"@es, "scénario de vidéo basé sur (expression)"@fr, "video screenplay based on (expression)"@en ;
    reg:hasSubproperty <http://rdaregistry.info/Elements/e/object/P20132> ;
    reg:hasUnconstrained <http://rdaregistry.info/Elements/u/P60234> ;
    reg:lexicalAlias <http://rdaregistry.info/Elements/e/videoScreenplayBasedOnExpression.en> ;
    reg:name "videoScreenplayBasedOnExpression"@en ;
    reg:status <http://metadataregistry.org/uri/RegStatus/1001> ;
    a rdf:Property ;
    rdfs:domain <http://rdaregistry.info/Elements/c/C10006> ;
    rdfs:isDefinedBy <http://rdaregistry.info/Elements/e/> ;
    rdfs:label "is video screenplay based on (expression)"@en ;
    rdfs:subPropertyOf <http://rdaregistry.info/Elements/e/P20129> ;
    skos:definition "Relates an expression to an expression of a work that has been adapted as a screenplay for a video."@en .

<http://rdaregistry.info/Elements/e/P20133>
    rdakit:instructionNumber "24.5" ;
    rdakit:toolkitDefinition "An expression of a work that has been adapted as a script for a radio program."@en, "Expression d’une œuvre qui a été adaptée en script d’émission de radio."@fr, "Una expresión de una obra que fue adaptada como el guión de un programa de radio."@es ;
    rdakit:toolkitLabel "guión radiofónico basado en (expresión)"@es, "radio script based on (expression)"@en, "script radiophonique basé sur (expression)"@fr ;
    reg:hasSubproperty <http://rdaregistry.info/Elements/e/object/P20133> ;
    reg:hasUnconstrained <http://rdaregistry.info/Elements/u/P60235> ;
    reg:lexicalAlias <http://rdaregistry.info/Elements/e/radioScriptBasedOnExpression.en> ;
    reg:name "radioScriptBasedOnExpression"@en ;
    reg:status <http://metadataregistry.org/uri/RegStatus/1001> ;
    a rdf:Property ;
    rdfs:domain <http://rdaregistry.info/Elements/c/C10006> ;
    rdfs:isDefinedBy <http://rdaregistry.info/Elements/e/> ;
    rdfs:label "is radio script based on (expression)"@en ;
    rdfs:subPropertyOf <http://rdaregistry.info/Elements/e/P20152> ;
    skos:definition "Relates an expression to an expression of a work that has been adapted as the script for a radio program."@en .

<http://rdaregistry.info/Elements/e/P20134>
    rdakit:instructionNumber "24.5" ;
    rdakit:toolkitDefinition "An expression of a work that has been adapted for video."@en, "Expression d’une œuvre qui a été adaptée en vidéo."@fr, "Una expresión de una obra que fue adaptada para video."@es ;
    rdakit:toolkitLabel "adaptación para video de (expresión)"@es, "adaptation en vidéo de (expression)"@fr, "video adaptation of (expression)"@en ;
    reg:hasSubproperty <http://rdaregistry.info/Elements/e/object/P20134> ;
    reg:hasUnconstrained <http://rdaregistry.info/Elements/u/P60236> ;
    reg:lexicalAlias <http://rdaregistry.info/Elements/e/videoAdaptationOfExpression.en> ;
    reg:name "videoAdaptationOfExpression"@en ;
    reg:status <http://metadataregistry.org/uri/RegStatus/1001> ;
    a rdf:Property ;
    rdfs:domain <http://rdaregistry.info/Elements/c/C10006> ;
    rdfs:isDefinedBy <http://rdaregistry.info/Elements/e/> ;
    rdfs:label "is video adaptation of (expression)"@en ;
    rdfs:subPropertyOf <http://rdaregistry.info/Elements/e/P20152> ;
    skos:definition "Relates an expression to an expression of a work that has been adapted for video."@en .

<http://rdaregistry.info/Elements/e/P20135>
    rdakit:instructionNumber "24.5" ;
    rdakit:toolkitDefinition "An expression of a work that has been digested, i.e., systematically and comprehensively condensed."@en, "Expression d’une œuvre qui a été condensée, c’est-à-dire abrégée de manière systématique et complète."@fr, "Una expresión de una obra que ha sido resumida, i.e., condensada sistemática e integralmente."@es ;
    rdakit:toolkitLabel "compendio de (expresión)"@es, "condensé de (expression)"@fr, "digest of (expression)"@en ;
    reg:hasSubproperty <http://rdaregistry.info/Elements/e/object/P20135> ;
    reg:hasUnconstrained <http://rdaregistry.info/Elements/u/P60238> ;
    reg:lexicalAlias <http://rdaregistry.info/Elements/e/digestOfExpression.en> ;
    reg:name "digestOfExpression"@en ;
    reg:status <http://metadataregistry.org/uri/RegStatus/1001> ;
    a rdf:Property ;
    rdfs:domain <http://rdaregistry.info/Elements/c/C10006> ;
    rdfs:isDefinedBy <http://rdaregistry.info/Elements/e/> ;
    rdfs:label "is digest of (expression)"@en ;
    rdfs:subPropertyOf <http://rdaregistry.info/Elements/e/P20204> ;
    skos:definition "Relates an expression to an expression of a work that has been digested, i.e., systematically and comprehensively condensed."@en .

<http://rdaregistry.info/Elements/e/P20136>
    reg:status <http://metadataregistry.org/uri/RegStatus/1008> ;
    a rdf:Property ;
    rdfs:isDefinedBy <http://rdaregistry.info/Elements/e/> ;
    rdfs:subPropertyOf <http://rdaregistry.info/Elements/e/P20072> .

<http://rdaregistry.info/Elements/e/P20137>
    rdakit:instructionNumber "24.5" ;
    rdakit:toolkitDefinition "An expression of a work that has been incorporated into another expression."@en, "Expression d’une œuvre qui a été intégrée dans une autre expression."@fr, "Una expresión de una obra que se ha incorporado en otra expresión."@es ;
    rdakit:toolkitLabel "absorción de (expresión)"@es, "absorption de (expression)"@fr, "absorption of (expression)"@en ;
    reg:hasSubproperty <http://rdaregistry.info/Elements/e/object/P20137> ;
    reg:hasUnconstrained <http://rdaregistry.info/Elements/u/P60574> ;
    reg:lexicalAlias <http://rdaregistry.info/Elements/e/absorptionOfExpression.en> ;
    reg:name "absorptionOfExpression"@en ;
    reg:status <http://metadataregistry.org/uri/RegStatus/1001> ;
    a rdf:Property ;
    rdfs:domain <http://rdaregistry.info/Elements/c/C10006> ;
    rdfs:isDefinedBy <http://rdaregistry.info/Elements/e/> ;
    rdfs:label "is absorption of (expression)"@en ;
    rdfs:subPropertyOf <http://rdaregistry.info/Elements/e/P20154> ;
    skos:definition "Relates an expression to an expression of a work that has been incorporated into another expression."@en .

<http://rdaregistry.info/Elements/e/P20138>
    rdakit:instructionNumber "24.5" ;
    rdakit:toolkitDefinition "An expression of a work that has been partially incorporated into another expression."@en, "Expression d’une œuvre qui a été partiellement intégrée dans une autre expression."@fr, "Una expresión de una obra que se ha incorporado parcialmente en otra expresión."@es ;
    rdakit:toolkitLabel "absorción en parte de (expresión)"@es, "absorption in part of (expression)"@en, "absorption partielle de (expression)"@fr ;
    reg:hasSubproperty <http://rdaregistry.info/Elements/e/object/P20138> ;
    reg:hasUnconstrained <http://rdaregistry.info/Elements/u/P60575> ;
    reg:lexicalAlias <http://rdaregistry.info/Elements/e/absorptionInPartOfExpression.en> ;
    reg:name "absorptionInPartOfExpression"@en ;
    reg:status <http://metadataregistry.org/uri/RegStatus/1001> ;
    a rdf:Property ;
    rdfs:domain <http://rdaregistry.info/Elements/c/C10006> ;
    rdfs:isDefinedBy <http://rdaregistry.info/Elements/e/> ;
    rdfs:label "is absorption in part of (expression)"@en ;
    rdfs:subPropertyOf <http://rdaregistry.info/Elements/e/P20154> ;
    skos:definition "Relates an expression to an expression of a work that has been partially incorporated into another expression."@en .

<http://rdaregistry.info/Elements/e/P20139>
    rdakit:instructionNumber "24.5" ;
    rdakit:toolkitDefinition "An expression of a musical work that has been rewritten for a medium of performance different from that for which the work was originally intended."@en, "Expression d’une œuvre qui a été réécrite pour une distribution d’exécution différente de celle à laquelle l’œuvre était destinée à l’origine."@fr, "Una expresión de una obra musical que fue reescrita para un medio de interpretación diferente de aquel para la que fue originalmente prevista."@es ;
    rdakit:toolkitLabel "arrangement de"@fr, "arrangement of"@en, "arreglo de"@es ;
    reg:hasSubproperty <http://rdaregistry.info/Elements/e/object/P20139> ;
    reg:hasUnconstrained <http://rdaregistry.info/Elements/u/P60242> ;
    reg:lexicalAlias <http://rdaregistry.info/Elements/e/arrangementOf.en> ;
    reg:name "arrangementOf"@en ;
    reg:status <http://metadataregistry.org/uri/RegStatus/1001> ;
    a rdf:Property ;
    rdfs:domain <http://rdaregistry.info/Elements/c/C10006> ;
    rdfs:isDefinedBy <http://rdaregistry.info/Elements/e/> ;
    rdfs:label "is arrangement of"@en ;
    rdfs:subPropertyOf <http://rdaregistry.info/Elements/e/P20204> ;
    skos:definition "Relates an expression to an expression of a musical work that has been rewritten for a medium of performance different from that for which the work was originally intended."@en .

<http://rdaregistry.info/Elements/e/P20140>
    rdakit:instructionNumber "24.5" ;
    rdakit:toolkitDefinition "An expression of a work that has been adapted and translated into another language."@en, "Expression d’une œuvre qui a été librement traduite en préservant l’esprit de l’original, mais non ses particularités linguistiques."@fr, "Una expresión de una obra que fue traducida libremente, preservando el espíritu del original, pero no sus detalles lingüísticos."@es ;
    rdakit:toolkitLabel "free translation of (expression)"@en, "traducción libre de (expresión)"@es, "traduction libre de (expression)"@fr ;
    reg:hasSubproperty <http://rdaregistry.info/Elements/e/object/P20140> ;
    reg:hasUnconstrained <http://rdaregistry.info/Elements/u/P60243> ;
    reg:lexicalAlias <http://rdaregistry.info/Elements/e/freeTranslationOfExpression.en> ;
    reg:name "freeTranslationOfExpression"@en ;
    reg:status <http://metadataregistry.org/uri/RegStatus/1001> ;
    a rdf:Property ;
    rdfs:domain <http://rdaregistry.info/Elements/c/C10006> ;
    rdfs:isDefinedBy <http://rdaregistry.info/Elements/e/> ;
    rdfs:label "is free translation of (expression)"@en ;
    rdfs:subPropertyOf <http://rdaregistry.info/Elements/e/P20204> ;
    skos:definition "Relates an expression to an expression of a work that has been adapted and translated into another language."@en .

<http://rdaregistry.info/Elements/e/P20141>
    rdakit:instructionNumber "24.5" ;
    rdakit:toolkitDefinition "An expression of a work that has been translated, i.e., the text expressed in a language different from that of an original work."@en, "Expression d’une œuvre qui a été traduite, c’est-à-dire dont le texte a été exprimé dans une langue différente de celle de l’œuvre d’origine."@fr, "Una expresión de una obra que fue traducida, i.e., el texto expresado en una lengua diferente de la utilizada en la obra original."@es ;
    rdakit:toolkitLabel "traducción de"@es, "traduction de"@fr, "translation of"@en ;
    reg:hasSubproperty <http://rdaregistry.info/Elements/e/P20078>, <http://rdaregistry.info/Elements/e/object/P20141> ;
    reg:hasUnconstrained <http://rdaregistry.info/Elements/u/P60244> ;
    reg:lexicalAlias <http://rdaregistry.info/Elements/e/translationOf.en> ;
    reg:name "translationOf"@en ;
    reg:status <http://metadataregistry.org/uri/RegStatus/1001> ;
    a rdf:Property ;
    rdfs:domain <http://rdaregistry.info/Elements/c/C10006> ;
    rdfs:isDefinedBy <http://rdaregistry.info/Elements/e/> ;
    rdfs:label "is translation of"@en ;
    rdfs:subPropertyOf <http://rdaregistry.info/Elements/e/P20204> ;
    skos:definition "Relates an expression to an expression of a work that has been translated, i.e., the text expressed in a language different from that of an original work."@en .

<http://rdaregistry.info/Elements/e/P20142>
    rdakit:instructionNumber "24.5" ;
    rdakit:toolkitDefinition "An expression of a work that imitates the style or content of a source work for comic effect."@en, "Expression d’une œuvre qui imite le style ou le contenu de l’œuvre source dans le but de produire un effet comique."@fr, "Una expresión de una obra que imita el estilo o contenido de la obra fuente para crear un efecto cómico."@es ;
    rdakit:toolkitLabel "parodiada como (expresión)"@es, "parodied as (expression)"@en, "parodié comme (expression)"@fr ;
    reg:hasSubproperty <http://rdaregistry.info/Elements/e/object/P20142> ;
    reg:hasUnconstrained <http://rdaregistry.info/Elements/u/P60246> ;
    reg:lexicalAlias <http://rdaregistry.info/Elements/e/parodiedAsExpression.en> ;
    reg:name "parodiedAsExpression"@en ;
    reg:status <http://metadataregistry.org/uri/RegStatus/1001> ;
    a rdf:Property ;
    rdfs:domain <http://rdaregistry.info/Elements/c/C10006> ;
    rdfs:isDefinedBy <http://rdaregistry.info/Elements/e/> ;
    rdfs:label "is parodied as (expression)"@en ;
    rdfs:subPropertyOf <http://rdaregistry.info/Elements/e/P20114> ;
    skos:definition "Relates an expression to an expression of a work that imitates the style or content of a source work for comic effect."@en .

<http://rdaregistry.info/Elements/e/P20143>
    rdakit:instructionNumber "24.5" ;
    rdakit:toolkitDefinition "An expression of a work that incorporates another expression."@en, "Expression d’une œuvre qui intègre une autre expression."@fr, "Una expresión de una obra que incorpora otra expresión."@es ;
    rdakit:toolkitLabel "absorbed by (expression)"@en, "absorbida por (expresión)"@es, "absorbé par (expression)"@fr ;
    reg:hasSubproperty <http://rdaregistry.info/Elements/e/object/P20143> ;
    reg:hasUnconstrained <http://rdaregistry.info/Elements/u/P60247> ;
    reg:lexicalAlias <http://rdaregistry.info/Elements/e/absorbedByExpression.en> ;
    reg:name "absorbedByExpression"@en ;
    reg:status <http://metadataregistry.org/uri/RegStatus/1001> ;
    a rdf:Property ;
    rdfs:domain <http://rdaregistry.info/Elements/c/C10006> ;
    rdfs:isDefinedBy <http://rdaregistry.info/Elements/e/> ;
    rdfs:label "is absorbed by (expression)"@en ;
    rdfs:subPropertyOf <http://rdaregistry.info/Elements/e/P20169> ;
    skos:definition "Relates an expression to an expression of a work that incorporates another expression."@en .

<http://rdaregistry.info/Elements/e/P20144>
    rdakit:instructionNumber "24.5" ;
    rdakit:toolkitDefinition "An expression of a work that incorporates part of the content of another expression."@en, "Expression d’une œuvre qui intègre une partie du contenu d’une autre expression."@fr, "Una expresión de una obra que incorpora parte del contenido de otra expresión."@es ;
    rdakit:toolkitLabel "absorbed in part by (expression)"@en, "absorbida en parte por (expresión)"@es, "absorbé en partie par (expression)"@fr ;
    reg:hasSubproperty <http://rdaregistry.info/Elements/e/object/P20144> ;
    reg:hasUnconstrained <http://rdaregistry.info/Elements/u/P60248> ;
    reg:lexicalAlias <http://rdaregistry.info/Elements/e/absorbedInPartByExpression.en> ;
    reg:name "absorbedInPartByExpression"@en ;
    reg:status <http://metadataregistry.org/uri/RegStatus/1001> ;
    a rdf:Property ;
    rdfs:domain <http://rdaregistry.info/Elements/c/C10006> ;
    rdfs:isDefinedBy <http://rdaregistry.info/Elements/e/> ;
    rdfs:label "is absorbed in part by (expression)"@en ;
    rdfs:subPropertyOf <http://rdaregistry.info/Elements/e/P20169> ;
    skos:definition "Relates an expression to an expression of a work that incorporates part of the content of another expression."@en .

<http://rdaregistry.info/Elements/e/P20145>
    rdakit:instructionNumber "24.5" ;
    rdakit:toolkitDefinition "An expression of a work that is a discrete component of a larger expression."@en, "Expression d’une œuvre qui est une composante distincte d’une expression plus vaste."@fr, "Una expresión de una obra que es un componente separado de una expresión mayor."@es ;
    rdakit:toolkitLabel "container of (expression)"@en, "conteneur de (expression)"@fr, "contiene (expresión)"@es ;
    reg:hasSubproperty <http://rdaregistry.info/Elements/e/object/P20145> ;
    reg:hasUnconstrained <http://rdaregistry.info/Elements/u/P60249> ;
    reg:lexicalAlias <http://rdaregistry.info/Elements/e/containerOfExpression.en> ;
    reg:name "containerOfExpression"@en ;
    reg:status <http://metadataregistry.org/uri/RegStatus/1001> ;
    a rdf:Property ;
    rdfs:domain <http://rdaregistry.info/Elements/c/C10006> ;
    rdfs:isDefinedBy <http://rdaregistry.info/Elements/e/> ;
    rdfs:label "is container of (expression)"@en ;
    rdfs:subPropertyOf <http://rdaregistry.info/Elements/e/P20236> ;
    skos:definition "Relates an expression to an expression of a work that is a discrete component of a larger expression."@en .

<http://rdaregistry.info/Elements/e/P20146>
    rdakit:instructionNumber "24.5" ;
    rdakit:toolkitDefinition "An expression of a work that is augmented by a list of errors in a predominant work, discovered after publication, with their corrections."@en, "Expression d’une œuvre qui est augmentée d’une liste d’erreurs dans l’œuvre prédominante, découvertes après publication, avec leurs corrections."@fr, "Una expresión de una obra que es aumentada por una lista de errores en la obra principal, descubiertos después de la publicación, con sus correcciones."@es ;
    rdakit:toolkitLabel "errata de (expression)"@fr, "errata to (expression)"@en, "fe de erratas de (expresión)"@es ;
    reg:hasSubproperty <http://rdaregistry.info/Elements/e/object/P20146> ;
    reg:hasUnconstrained <http://rdaregistry.info/Elements/u/P60251> ;
    reg:lexicalAlias <http://rdaregistry.info/Elements/e/errataToExpression.en> ;
    reg:name "errataToExpression"@en ;
    reg:status <http://metadataregistry.org/uri/RegStatus/1001> ;
    a rdf:Property ;
    rdfs:domain <http://rdaregistry.info/Elements/c/C10006> ;
    rdfs:isDefinedBy <http://rdaregistry.info/Elements/e/> ;
    rdfs:label "is errata to (expression)"@en ;
    rdfs:subPropertyOf <http://rdaregistry.info/Elements/e/P20192> ;
    skos:definition "Relates an expression to an expression of a work that is augmented by a list of errors in a predominant work, discovered after publication, with their corrections."@en .

<http://rdaregistry.info/Elements/e/P20147>
    rdakit:instructionNumber "24.5" ;
    rdakit:toolkitDefinition "An expression of a work that is augmented by another work consisting of material to help the user of a predominant work, such as notes, learning and study aids, exercises, problems, questions and answers, instructor or student materials, etc."@en, "Expression d’une œuvre qui est augmentée par une autre œuvre consistant en documentation destinée à aider l’utilisateur de l’œuvre prédominante, telle que des notes, des outils pédagogiques, des exercices, des problèmes, des questions et réponses, du matériel didactique, etc."@fr, "Una expresión de una obra que es aumentada por otra obra que consiste en material de ayuda para el usuario de la obra principal, tal como notas, ayudas de aprendizaje y estudio, ejercicios, problemas, preguntas y respuestas, materiales para el instructor y el estudiante, etc."@es ;
    rdakit:toolkitLabel "guide de (expression)"@fr, "guide to (expression)"@en, "guía de (expresión)"@es ;
    reg:hasSubproperty <http://rdaregistry.info/Elements/e/object/P20147> ;
    reg:hasUnconstrained <http://rdaregistry.info/Elements/u/P60252> ;
    reg:lexicalAlias <http://rdaregistry.info/Elements/e/guideToExpression.en> ;
    reg:name "guideToExpression"@en ;
    reg:status <http://metadataregistry.org/uri/RegStatus/1001> ;
    a rdf:Property ;
    rdfs:domain <http://rdaregistry.info/Elements/c/C10006> ;
    rdfs:isDefinedBy <http://rdaregistry.info/Elements/e/> ;
    rdfs:label "is guide to (expression)"@en ;
    rdfs:subPropertyOf <http://rdaregistry.info/Elements/e/P20192> ;
    skos:definition "Relates an expression to an expression of a work that is augmented by another work consisting of material to help the user of a predominant work, such as notes, learning and study aids, exercises, problems, questions and answers, instructor or student materials, etc."@en .

<http://rdaregistry.info/Elements/e/P20148>
    rdakit:instructionNumber "24.5" ;
    rdakit:toolkitDefinition "An expression of a work that is augmented by pictorial content designed to explain or decorate it."@en, "Expression d’une œuvre qui est augmentée par du contenu visuel destiné à l’expliquer ou à la décorer."@fr, "Una expresión de una obra que es aumentada con contenido pictórico diseñado para explicarla o decorarla."@es ;
    rdakit:toolkitLabel "illustrations for (expression)"@en, "illustrations pour (expression)"@fr, "ilustraciones para (expresión)"@es ;
    reg:hasSubproperty <http://rdaregistry.info/Elements/e/object/P20148> ;
    reg:hasUnconstrained <http://rdaregistry.info/Elements/u/P60254> ;
    reg:lexicalAlias <http://rdaregistry.info/Elements/e/illustrationsForExpression.en> ;
    reg:name "illustrationsForExpression"@en ;
    reg:status <http://metadataregistry.org/uri/RegStatus/1001> ;
    a rdf:Property ;
    rdfs:domain <http://rdaregistry.info/Elements/c/C10006> ;
    rdfs:isDefinedBy <http://rdaregistry.info/Elements/e/> ;
    rdfs:label "is illustrations for (expression)"@en ;
    rdfs:subPropertyOf <http://rdaregistry.info/Elements/e/P20192> ;
    skos:definition "Relates an expression to an expression of a work that is augmented by pictorial content designed to explain or decorate it."@en .

<http://rdaregistry.info/Elements/e/P20149>
    rdakit:instructionNumber "24.5" ;
    rdakit:toolkitDefinition "An expression of a work that is continued by the content of an expression of a later work."@en, "Expression d’une œuvre qui est continuée par le contenu d’une expression d’une œuvre ultérieure."@fr, "Una expresión de una obra que es continuada por el contenido de una expresión de una obra posterior."@es ;
    rdakit:toolkitLabel "continuación de (expresión)"@es, "continuation de (expression)"@fr, "continuation of (expression)"@en ;
    reg:hasSubproperty <http://rdaregistry.info/Elements/e/object/P20149> ;
    reg:hasUnconstrained <http://rdaregistry.info/Elements/u/P60576> ;
    reg:lexicalAlias <http://rdaregistry.info/Elements/e/continuationOfExpression.en> ;
    reg:name "continuationOfExpression"@en ;
    reg:status <http://metadataregistry.org/uri/RegStatus/1001> ;
    a rdf:Property ;
    rdfs:domain <http://rdaregistry.info/Elements/c/C10006> ;
    rdfs:isDefinedBy <http://rdaregistry.info/Elements/e/> ;
    rdfs:label "is continuation of (expression)"@en ;
    rdfs:subPropertyOf <http://rdaregistry.info/Elements/e/P20154> ;
    skos:definition "Relates an expression to an expression of a work that is continued by the content of an expression of a later work."@en ;
    skos:scopeNote "This relationship applies generally to serials."@en .

<http://rdaregistry.info/Elements/e/P20150>
    reg:status <http://metadataregistry.org/uri/RegStatus/1008> ;
    a rdf:Property ;
    rdfs:isDefinedBy <http://rdaregistry.info/Elements/e/> ;
    rdfs:subPropertyOf <http://rdaregistry.info/Elements/e/P20072> .

<http://rdaregistry.info/Elements/e/P20151>
    rdakit:instructionNumber "24.5" ;
    rdakit:toolkitDefinition "An expression of a work that is updated or otherwise complemented by an augmenting expression."@en, "Expression d’une œuvre qui est mise à jour ou complétée d’une autre façon par l’expression augmentante."@fr, "Una expresión de una obra que es actualizada o complementada por la expresión que aumenta."@es ;
    rdakit:toolkitLabel "suplemento de (expresión)"@es, "supplement to (expression)"@en, "supplément de (expression)"@fr ;
    reg:hasSubproperty <http://rdaregistry.info/Elements/e/object/P20151> ;
    reg:hasUnconstrained <http://rdaregistry.info/Elements/u/P60259> ;
    reg:lexicalAlias <http://rdaregistry.info/Elements/e/supplementToExpression.en> ;
    reg:name "supplementToExpression"@en ;
    reg:status <http://metadataregistry.org/uri/RegStatus/1001> ;
    a rdf:Property ;
    rdfs:domain <http://rdaregistry.info/Elements/c/C10006> ;
    rdfs:isDefinedBy <http://rdaregistry.info/Elements/e/> ;
    rdfs:label "is supplement to (expression)"@en ;
    rdfs:subPropertyOf <http://rdaregistry.info/Elements/e/P20192> ;
    skos:definition "Relates an expression to an expression of a work that is updated or otherwise complemented by an augmenting expression."@en .

<http://rdaregistry.info/Elements/e/P20152>
    rdakit:instructionNumber "24.5" ;
    rdakit:toolkitDefinition "An expression of a work that has been modified for a purpose, use, or medium other than that for which it was originally intended."@en, "Expression d’une œuvre qui a été modifiée pour une fin, une utilisation ou un mode d’expression autre que celui auquel elle était destinée à l’origine."@fr, "Una expresión de una obra que ha sido modificada para un propósito, uso o medio diferente del previsto originalmente."@es ;
    rdakit:toolkitLabel "adaptación de (expresión)"@es, "adaptation de (expression)"@fr, "adaptation of (expression)"@en ;
    reg:hasSubproperty <http://rdaregistry.info/Elements/e/P20123>, <http://rdaregistry.info/Elements/e/P20124>, <http://rdaregistry.info/Elements/e/P20125>, <http://rdaregistry.info/Elements/e/P20126>, <http://rdaregistry.info/Elements/e/P20127>, <http://rdaregistry.info/Elements/e/P20128>, <http://rdaregistry.info/Elements/e/P20129>, <http://rdaregistry.info/Elements/e/P20133>, <http://rdaregistry.info/Elements/e/P20134>, <http://rdaregistry.info/Elements/e/P20256>, <http://rdaregistry.info/Elements/e/P20281>, <http://rdaregistry.info/Elements/e/object/P20152> ;
    reg:hasUnconstrained <http://rdaregistry.info/Elements/u/P60241> ;
    reg:lexicalAlias <http://rdaregistry.info/Elements/e/adaptationOfExpression.en> ;
    reg:name "adaptationOfExpression"@en ;
    reg:status <http://metadataregistry.org/uri/RegStatus/1001> ;
    a rdf:Property ;
    rdfs:domain <http://rdaregistry.info/Elements/c/C10006> ;
    rdfs:isDefinedBy <http://rdaregistry.info/Elements/e/> ;
    rdfs:label "is adaptation of (expression)"@en ;
    rdfs:subPropertyOf <http://rdaregistry.info/Elements/e/P20204> ;
    skos:definition "Relates an expression to an expression of a work that has been modified for a purpose, use, or medium other than that for which it was originally intended."@en .

<http://rdaregistry.info/Elements/e/P20153>
    rdakit:instructionNumber "24.5" ;
    rdakit:toolkitDefinition "An expression of a work that modifies a source expression for a purpose, use, or medium other than that for which it was originally intended."@en, "Expression d’une œuvre qui modifie l’expression source pour une fin, une utilisation ou un mode d’expression autre que celui auquel elle était destinée à l’origine."@fr, "Una expresión de una obra que modifica la expresión fuente para un propósito, uso o medio diferente del previsto originalmente."@es ;
    rdakit:toolkitLabel "adaptada como (expresión)"@es, "adapted as (expression)"@en, "adapté comme (expression)"@fr ;
    reg:hasSubproperty <http://rdaregistry.info/Elements/e/P20009>, <http://rdaregistry.info/Elements/e/P20060>, <http://rdaregistry.info/Elements/e/P20066>, <http://rdaregistry.info/Elements/e/P20067>, <http://rdaregistry.info/Elements/e/P20073>, <http://rdaregistry.info/Elements/e/P20077>, <http://rdaregistry.info/Elements/e/P20088>, <http://rdaregistry.info/Elements/e/P20096>, <http://rdaregistry.info/Elements/e/P20099>, <http://rdaregistry.info/Elements/e/P20255>, <http://rdaregistry.info/Elements/e/P20282>, <http://rdaregistry.info/Elements/e/object/P20153> ;
    reg:hasUnconstrained <http://rdaregistry.info/Elements/u/P60260> ;
    reg:lexicalAlias <http://rdaregistry.info/Elements/e/adaptedAsExpression.en> ;
    reg:name "adaptedAsExpression"@en ;
    reg:status <http://metadataregistry.org/uri/RegStatus/1001> ;
    a rdf:Property ;
    rdfs:domain <http://rdaregistry.info/Elements/c/C10006> ;
    rdfs:isDefinedBy <http://rdaregistry.info/Elements/e/> ;
    rdfs:label "is adapted as (expression)"@en ;
    rdfs:subPropertyOf <http://rdaregistry.info/Elements/e/P20203> ;
    skos:definition "Relates an expression to an expression of a work based on a source expression."@en .

<http://rdaregistry.info/Elements/e/P20154>
    rdakit:instructionNumber "24.5" ;
    rdakit:toolkitDefinition "An expression of a work that precedes, that is, is earlier in time or before in narrative, etc., a succeeding expression."@en, "Expression d’une œuvre qui précède l’expression suivante (par exemple, qui lui est antérieure dans le temps ou dans un récit)."@fr, "Una expresión de una obra que precede (por ej., es anterior en el tiempo o en la narración) la expresión que sigue."@es ;
    rdakit:toolkitLabel "preceded by (expression)"@en, "precedida por (expresión)"@es, "précédé de (expression)"@fr ;
    reg:hasSubproperty <http://rdaregistry.info/Elements/e/P20137>, <http://rdaregistry.info/Elements/e/P20138>, <http://rdaregistry.info/Elements/e/P20149>, <http://rdaregistry.info/Elements/e/P20167>, <http://rdaregistry.info/Elements/e/P20168>, <http://rdaregistry.info/Elements/e/P20198>, <http://rdaregistry.info/Elements/e/P20199>, <http://rdaregistry.info/Elements/e/P20201>, <http://rdaregistry.info/Elements/e/object/P20154> ;
    reg:hasUnconstrained <http://rdaregistry.info/Elements/u/P60261> ;
    reg:lexicalAlias <http://rdaregistry.info/Elements/e/precededByExpression.en> ;
    reg:name "precededByExpression"@en ;
    reg:status <http://metadataregistry.org/uri/RegStatus/1001> ;
    a rdf:Property ;
    rdfs:domain <http://rdaregistry.info/Elements/c/C10006> ;
    rdfs:isDefinedBy <http://rdaregistry.info/Elements/e/> ;
    rdfs:label "is preceded by (expression)"@en ;
    rdfs:subPropertyOf <http://rdaregistry.info/Elements/e/P20235> ;
    skos:definition "Relates an expression to an expression of a work that precedes, that is, is earlier in time or before in narrative, etc., a succeeding expression."@en .

<http://rdaregistry.info/Elements/e/P20155>
    rdakit:instructionNumber "24.5" ;
    rdakit:toolkitDefinition "An expression of a work that provides a guide to the organization, arrangement, and contents of an archival collection."@en, "Expression d’une œuvre qui fournit un guide de l’organisation, du classement et du contenu d’une collection ou d’un fonds d’archives."@fr, "Una expresión de una obra que proporciona una guía para la organización, ordenación y contenido de una colección archivística."@es ;
    rdakit:toolkitLabel "finding aid (expression)"@en, "guía de búsqueda (expresión)"@es, "instrument de recherche (expression)"@fr ;
    reg:hasSubproperty <http://rdaregistry.info/Elements/e/object/P20155> ;
    reg:hasUnconstrained <http://rdaregistry.info/Elements/u/P60262> ;
    reg:lexicalAlias <http://rdaregistry.info/Elements/e/findingAidExpression.en> ;
    reg:name "findingAidExpression"@en ;
    reg:status <http://metadataregistry.org/uri/RegStatus/1001> ;
    a rdf:Property ;
    rdfs:domain <http://rdaregistry.info/Elements/c/C10006> ;
    rdfs:isDefinedBy <http://rdaregistry.info/Elements/e/> ;
    rdfs:label "is finding aid (expression)"@en ;
    rdfs:subPropertyOf <http://rdaregistry.info/Elements/e/P20105> ;
    skos:definition "Relates an expression to an expression of a work that provides a guide to the organization, arrangement, and contents of an archival collection."@en .

<http://rdaregistry.info/Elements/e/P20156>
    rdakit:instructionNumber "24.5" ;
    rdakit:toolkitDefinition "An expression of a work that provides a systematic, alphabetical guide to the contents of a predominant expression, usually keyed to page numbers or other reference codes."@en, "Expression d’une œuvre qui fournit un guide méthodique et alphabétique du contenu de l’expression prédominante, renvoyant généralement à des numéros de page ou à d’autres codes de référence."@fr, "Una expresión de una obra que proporciona una guía alfabética y sistemática al contenido de la entidad principal, generalmente indicando los números de página u otros códigos de referencia."@es ;
    rdakit:toolkitLabel "index (expression)"@en, "index (expression)"@fr, "índice (expresión)"@es ;
    reg:hasSubproperty <http://rdaregistry.info/Elements/e/object/P20156> ;
    reg:hasUnconstrained <http://rdaregistry.info/Elements/u/P60263> ;
    reg:lexicalAlias <http://rdaregistry.info/Elements/e/indexExpression.en> ;
    reg:name "indexExpression"@en ;
    reg:status <http://metadataregistry.org/uri/RegStatus/1001> ;
    a rdf:Property ;
    rdfs:domain <http://rdaregistry.info/Elements/c/C10006> ;
    rdfs:isDefinedBy <http://rdaregistry.info/Elements/e/> ;
    rdfs:label "is index (expression)"@en ;
    rdfs:subPropertyOf <http://rdaregistry.info/Elements/e/P20105> ;
    skos:definition "Relates an expression to an expression of a work that provides a systematic, alphabetical guide to the contents of a predominant expression, usually keyed to page numbers or other reference codes."@en .

<http://rdaregistry.info/Elements/e/P20157>
    rdakit:instructionNumber "24.5" ;
    rdakit:toolkitDefinition "An expression of a work that provides text for a motion picture, television program or video."@en, "Expression d’une œuvre qui fournit le texte d’un film, d’une émission de télévision ou d’une vidéo."@fr, "Una expresión de una obra que proporciona el texto para una película cinematográfica, programa de televisión o video."@es ;
    rdakit:toolkitLabel "guión (expresión)"@es, "screenplay (expression)"@en, "scénario (expression)"@fr ;
    reg:hasSubproperty <http://rdaregistry.info/Elements/e/P20158>, <http://rdaregistry.info/Elements/e/P20161>, <http://rdaregistry.info/Elements/e/P20162>, <http://rdaregistry.info/Elements/e/object/P20157> ;
    reg:hasUnconstrained <http://rdaregistry.info/Elements/u/P60264> ;
    reg:lexicalAlias <http://rdaregistry.info/Elements/e/screenplayExpression.en> ;
    reg:name "screenplayExpression"@en ;
    reg:status <http://metadataregistry.org/uri/RegStatus/1001> ;
    a rdf:Property ;
    rdfs:domain <http://rdaregistry.info/Elements/c/C10006> ;
    rdfs:isDefinedBy <http://rdaregistry.info/Elements/e/> ;
    rdfs:label "is screenplay (expression)"@en ;
    rdfs:subPropertyOf <http://rdaregistry.info/Elements/e/P20100> ;
    skos:definition "Relates an expression to an expression of a work that provides text for a motion picture, television program or video."@en .

<http://rdaregistry.info/Elements/e/P20158>
    rdakit:instructionNumber "24.5" ;
    rdakit:toolkitDefinition "An expression of a work that provides text for a motion picture."@en, "Expression d’une œuvre qui fournit le texte d’un film."@fr, "Una expresión de una obra que proporciona el texto para una película cinematográfica."@es ;
    rdakit:toolkitLabel "guión cinematográfico (expresión)"@es, "motion picture screenplay (expression)"@en, "scénario de film (expression)"@fr ;
    reg:hasSubproperty <http://rdaregistry.info/Elements/e/object/P20158> ;
    reg:hasUnconstrained <http://rdaregistry.info/Elements/u/P60265> ;
    reg:lexicalAlias <http://rdaregistry.info/Elements/e/motionPictureScreenplayExpression.en> ;
    reg:name "motionPictureScreenplayExpression"@en ;
    reg:status <http://metadataregistry.org/uri/RegStatus/1001> ;
    a rdf:Property ;
    rdfs:domain <http://rdaregistry.info/Elements/c/C10006> ;
    rdfs:isDefinedBy <http://rdaregistry.info/Elements/e/> ;
    rdfs:label "is motion picture screenplay (expression)"@en ;
    rdfs:subPropertyOf <http://rdaregistry.info/Elements/e/P20157> ;
    skos:definition "Relates an expression to an expression of a work that provides text for a motion picture."@en .

<http://rdaregistry.info/Elements/e/P20159>
    rdakit:instructionNumber "24.5" ;
    rdakit:toolkitDefinition "An expression of a work that provides text for a non-dramatic musical work, other than an oratorio."@en, "Expression d’une œuvre qui fournit le texte d’une œuvre musicale non théâtrale, autre qu’un oratorio."@fr, "Una expresión de una obra que proporciona el texto de una obra musical no dramática, diferente de un oratorio."@es ;
    rdakit:toolkitLabel "composición musical de (expresión)"@es, "mise en musique de (expression)"@fr, "musical setting of (expression)"@en ;
    reg:hasSubproperty <http://rdaregistry.info/Elements/e/object/P20159> ;
    reg:hasUnconstrained <http://rdaregistry.info/Elements/u/P60266> ;
    reg:lexicalAlias <http://rdaregistry.info/Elements/e/musicalSettingOfExpression.en> ;
    reg:name "musicalSettingOfExpression"@en ;
    reg:status <http://metadataregistry.org/uri/RegStatus/1001> ;
    a rdf:Property ;
    rdfs:domain <http://rdaregistry.info/Elements/c/C10006> ;
    rdfs:isDefinedBy <http://rdaregistry.info/Elements/e/> ;
    rdfs:label "is musical setting of (expression)"@en ;
    rdfs:subPropertyOf <http://rdaregistry.info/Elements/e/P20204> ;
    skos:definition "Relates an expression to an expression of a work that provides text for a non-dramatic musical work, other than an oratorio."@en .

<http://rdaregistry.info/Elements/e/P20160>
    rdakit:instructionNumber "24.5" ;
    rdakit:toolkitDefinition "An expression of a work that provides text for a radio program."@en, "Expression d’une œuvre qui fournit le texte d’une émission de radio."@fr, "Una expresión de una obra que proporciona el texto para un programa de radio."@es ;
    rdakit:toolkitLabel "guión radiofónico (expresión)"@es, "radio script (expression)"@en, "script radiophonique (expression)"@fr ;
    reg:hasSubproperty <http://rdaregistry.info/Elements/e/object/P20160> ;
    reg:hasUnconstrained <http://rdaregistry.info/Elements/u/P60267> ;
    reg:lexicalAlias <http://rdaregistry.info/Elements/e/radioScriptExpression.en> ;
    reg:name "radioScriptExpression"@en ;
    reg:status <http://metadataregistry.org/uri/RegStatus/1001> ;
    a rdf:Property ;
    rdfs:domain <http://rdaregistry.info/Elements/c/C10006> ;
    rdfs:isDefinedBy <http://rdaregistry.info/Elements/e/> ;
    rdfs:label "is radio script (expression)"@en ;
    rdfs:subPropertyOf <http://rdaregistry.info/Elements/e/P20100> ;
    skos:definition "Relates an expression to an expression of a work that provides text for a radio program."@en .

<http://rdaregistry.info/Elements/e/P20161>
    rdakit:instructionNumber "24.5" ;
    rdakit:toolkitDefinition "An expression of a work that provides text for a television program."@en, "Expression d’une œuvre qui fournit le texte d’une émission de télévision."@fr, "Una expresión de una obra que proporciona el texto para un programa de televisión."@es ;
    rdakit:toolkitLabel "guión para televisión (expresión) Una"@es, "scénario de télévision (expression)"@fr, "television screenplay (expression)"@en ;
    reg:hasSubproperty <http://rdaregistry.info/Elements/e/object/P20161> ;
    reg:hasUnconstrained <http://rdaregistry.info/Elements/u/P60268> ;
    reg:lexicalAlias <http://rdaregistry.info/Elements/e/televisionScreenplayExpression.en> ;
    reg:name "televisionScreenplayExpression"@en ;
    reg:status <http://metadataregistry.org/uri/RegStatus/1001> ;
    a rdf:Property ;
    rdfs:domain <http://rdaregistry.info/Elements/c/C10006> ;
    rdfs:isDefinedBy <http://rdaregistry.info/Elements/e/> ;
    rdfs:label "is television screenplay (expression)"@en ;
    rdfs:subPropertyOf <http://rdaregistry.info/Elements/e/P20157> ;
    skos:definition "Relates an expression to an expression of a work that provides text for a television program."@en .

<http://rdaregistry.info/Elements/e/P20162>
    rdakit:instructionNumber "24.5" ;
    rdakit:toolkitDefinition "An expression of a work that provides text for a video."@en, "Expression d’une œuvre qui fournit le texte d’une vidéo."@fr, "Una expresión de una obra que proporciona el texto para un video."@es ;
    rdakit:toolkitLabel "guión para video (expresión)"@es, "scénario de vidéo (expression)"@fr, "video screenplay (expression)"@en ;
    reg:hasSubproperty <http://rdaregistry.info/Elements/e/object/P20162> ;
    reg:hasUnconstrained <http://rdaregistry.info/Elements/u/P60269> ;
    reg:lexicalAlias <http://rdaregistry.info/Elements/e/videoScreenplayExpression.en> ;
    reg:name "videoScreenplayExpression"@en ;
    reg:status <http://metadataregistry.org/uri/RegStatus/1001> ;
    a rdf:Property ;
    rdfs:domain <http://rdaregistry.info/Elements/c/C10006> ;
    rdfs:isDefinedBy <http://rdaregistry.info/Elements/e/> ;
    rdfs:label "is video screenplay (expression)"@en ;
    rdfs:subPropertyOf <http://rdaregistry.info/Elements/e/P20157> ;
    skos:definition "Relates an expression to an expression of a work that provides text for a video."@en .

<http://rdaregistry.info/Elements/e/P20163>
    rdakit:instructionNumber "24.5" ;
    rdakit:toolkitDefinition "An expression of a work that provides the text of an opera or other work for the musical stage, or an oratorio."@en, "Expression d’une œuvre qui fournit le texte d’un opéra ou d’une autre œuvre pour la scène musicale, ou bien d’un oratorio."@fr, "Una expresión de una obra que proporciona el texto de una ópera u otra obra para representación musical, o un oratorio."@es ;
    rdakit:toolkitLabel "libreto (expresión)"@es, "libretto (expression)"@en, "livret (expression)"@fr ;
    reg:hasSubproperty <http://rdaregistry.info/Elements/e/object/P20163> ;
    reg:hasUnconstrained <http://rdaregistry.info/Elements/u/P60270> ;
    reg:lexicalAlias <http://rdaregistry.info/Elements/e/librettoExpression.en> ;
    reg:name "librettoExpression"@en ;
    reg:status <http://metadataregistry.org/uri/RegStatus/1001> ;
    a rdf:Property ;
    rdfs:domain <http://rdaregistry.info/Elements/c/C10006> ;
    rdfs:isDefinedBy <http://rdaregistry.info/Elements/e/> ;
    rdfs:label "is libretto (expression)"@en ;
    rdfs:subPropertyOf <http://rdaregistry.info/Elements/e/P20100> ;
    skos:definition "Relates an expression to an expression of a work that provides the text of an opera or other work for the musical stage, or an oratorio."@en .

<http://rdaregistry.info/Elements/e/P20164>
    rdakit:instructionNumber "24.5" ;
    rdakit:toolkitDefinition "An expression of a work that restates the content of a source work in a different form."@en, "Expression d’une œuvre qui reprend le contenu de l’œuvre source sous une formulation différente."@fr, "Una expresión de una obra que replantea el contenido de una obra fuente en una forma diferente."@es ;
    rdakit:toolkitLabel "parafraseada como (expresión)"@es, "paraphrased as (expression)"@en, "paraphrasé comme (expression)"@fr ;
    reg:hasSubproperty <http://rdaregistry.info/Elements/e/object/P20164> ;
    reg:hasUnconstrained <http://rdaregistry.info/Elements/u/P60273> ;
    reg:lexicalAlias <http://rdaregistry.info/Elements/e/paraphrasedAsExpression.en> ;
    reg:name "paraphrasedAsExpression"@en ;
    reg:status <http://metadataregistry.org/uri/RegStatus/1001> ;
    a rdf:Property ;
    rdfs:domain <http://rdaregistry.info/Elements/c/C10006> ;
    rdfs:isDefinedBy <http://rdaregistry.info/Elements/e/> ;
    rdfs:label "is paraphrased as (expression)"@en ;
    rdfs:subPropertyOf <http://rdaregistry.info/Elements/e/P20203> ;
    skos:definition "Relates an expression to an expression of a work that restates the content of a source work in a different form."@en .

<http://rdaregistry.info/Elements/e/P20165>
    rdakit:instructionNumber "24.5" ;
    rdakit:toolkitDefinition "An expression of a musical work that rewrites a source expression for a medium of performance different from that for which the work was originally intended."@en, "Expression d’une œuvre musicale qui réécrit l’expression source pour une distribution d’exécution différente de celle à laquelle l’œuvre était destinée à l’origine."@fr, "Una expresión de una obra que reescribe la expresión fuente para un medio de interpretación diferente de aquel para el cual fue prevista originalmente."@es ;
    rdakit:toolkitLabel "arranged as"@en, "arrangé comme"@fr, "arreglada como"@es ;
    reg:hasSubproperty <http://rdaregistry.info/Elements/e/object/P20165> ;
    reg:hasUnconstrained <http://rdaregistry.info/Elements/u/P60274> ;
    reg:lexicalAlias <http://rdaregistry.info/Elements/e/arrangedAs.en> ;
    reg:name "arrangedAs"@en ;
    reg:status <http://metadataregistry.org/uri/RegStatus/1001> ;
    a rdf:Property ;
    rdfs:domain <http://rdaregistry.info/Elements/c/C10006> ;
    rdfs:isDefinedBy <http://rdaregistry.info/Elements/e/> ;
    rdfs:label "is arranged as"@en ;
    rdfs:subPropertyOf <http://rdaregistry.info/Elements/e/P20203> ;
    skos:definition "Relates an expression to an expression of a musical work that rewrites a source expression for a medium of performance different from that for which the work was originally intended."@en .

<http://rdaregistry.info/Elements/e/P20166>
    rdakit:instructionNumber "24.5" ;
    rdakit:toolkitDefinition "An expression of a work that shortens a source expression without changing the general meaning or manner of presentation."@en, "Expression d’une œuvre qui raccourcit l’expression source sans en changer le sens général ou le mode de présentation."@fr, "Una expresión de una obra que acorta la entidad fuente sin cambiar el sentido general o la forma de presentación."@es ;
    rdakit:toolkitLabel "abreviada como (expresión)"@es, "abridged as (expression)"@en, "abrégé comme (expression)"@fr ;
    reg:hasSubproperty <http://rdaregistry.info/Elements/e/object/P20166> ;
    reg:hasUnconstrained <http://rdaregistry.info/Elements/u/P60275> ;
    reg:lexicalAlias <http://rdaregistry.info/Elements/e/abridgedAsExpression.en> ;
    reg:name "abridgedAsExpression"@en ;
    reg:status <http://metadataregistry.org/uri/RegStatus/1001> ;
    a rdf:Property ;
    rdfs:domain <http://rdaregistry.info/Elements/c/C10006> ;
    rdfs:isDefinedBy <http://rdaregistry.info/Elements/e/> ;
    rdfs:label "is abridged as (expression)"@en ;
    rdfs:subPropertyOf <http://rdaregistry.info/Elements/e/P20203> ;
    skos:definition "Relates an expression to an expression of a work that shortens a source expression without changing the general meaning or manner of presentation."@en .

<http://rdaregistry.info/Elements/e/P20167>
    rdakit:instructionNumber "24.5" ;
    rdakit:toolkitDefinition "An expression of a work that split into two or more separate expressions with new titles."@en, "Expression d’une œuvre qui s’est scindée en deux ou plusieurs expressions distinctes avec de nouveaux titres."@fr, "Una expresión de una obra que se divide en dos o más entidades separadas con nuevos títulos."@es ;
    rdakit:toolkitLabel "continuation in part of (expression)"@en, "continuation partielle de (expression)"@fr, "continúa en parte (expresión)"@es ;
    reg:hasSubproperty <http://rdaregistry.info/Elements/e/object/P20167> ;
    reg:hasUnconstrained <http://rdaregistry.info/Elements/u/P60276> ;
    reg:lexicalAlias <http://rdaregistry.info/Elements/e/continuationInPartOfExpression.en> ;
    reg:name "continuationInPartOfExpression"@en ;
    reg:status <http://metadataregistry.org/uri/RegStatus/1001> ;
    a rdf:Property ;
    rdfs:domain <http://rdaregistry.info/Elements/c/C10006> ;
    rdfs:isDefinedBy <http://rdaregistry.info/Elements/e/> ;
    rdfs:label "is continuation in part of (expression)"@en ;
    rdfs:subPropertyOf <http://rdaregistry.info/Elements/e/P20154> ;
    skos:definition "Relates an expression to an expression of a work that split into two or more separate expressions with new titles."@en ;
    skos:scopeNote "This relationship applies generally to serials."@en .

<http://rdaregistry.info/Elements/e/P20168>
    rdakit:instructionNumber "24.5" ;
    rdakit:toolkitDefinition "An expression of a work that spun off a part of its content to form a new expression."@en, "Expression d’une œuvre dont une partie du contenu a été détachée pour former une nouvelle expression."@fr, "Una expresión de una obra que se desprende de una parte de su contenido para formar una expresión nueva."@es ;
    rdakit:toolkitLabel "scission de (expression)"@fr, "separada de (expresión)"@es, "separated from (expression)"@en ;
    reg:hasSubproperty <http://rdaregistry.info/Elements/e/object/P20168> ;
    reg:hasUnconstrained <http://rdaregistry.info/Elements/u/P60277> ;
    reg:lexicalAlias <http://rdaregistry.info/Elements/e/separatedFromExpression.en> ;
    reg:name "separatedFromExpression"@en ;
    reg:status <http://metadataregistry.org/uri/RegStatus/1001> ;
    a rdf:Property ;
    rdfs:domain <http://rdaregistry.info/Elements/c/C10006> ;
    rdfs:isDefinedBy <http://rdaregistry.info/Elements/e/> ;
    rdfs:label "is separated from (expression)"@en ;
    rdfs:subPropertyOf <http://rdaregistry.info/Elements/e/P20154> ;
    skos:definition "Relates an expression to an expression of a work that spun off a part of its content to form a new expression."@en .

<http://rdaregistry.info/Elements/e/P20169>
    rdakit:instructionNumber "24.5" ;
    rdakit:toolkitDefinition "An expression of a work that succeeds, that is, is later in time or after in a narrative, etc., a preceding expression."@en, "Expression d’une œuvre qui succède à l’expression précédente (par exemple, qui lui est ultérieure dans le temps ou dans un récit)."@fr, "Una expresión de una obra que sucede a (por ej., posterior en el tiempo o posterior en una narración) la expresión predecesora."@es ;
    rdakit:toolkitLabel "seguida por (expresión)"@es, "succeeded by (expression)"@en, "suivi de (expression)"@fr ;
    reg:hasSubproperty <http://rdaregistry.info/Elements/e/P20075>, <http://rdaregistry.info/Elements/e/P20076>, <http://rdaregistry.info/Elements/e/P20101>, <http://rdaregistry.info/Elements/e/P20143>, <http://rdaregistry.info/Elements/e/P20144>, <http://rdaregistry.info/Elements/e/P20191>, <http://rdaregistry.info/Elements/e/P20200>, <http://rdaregistry.info/Elements/e/P20212>, <http://rdaregistry.info/Elements/e/object/P20169> ;
    reg:hasUnconstrained <http://rdaregistry.info/Elements/u/P60278> ;
    reg:lexicalAlias <http://rdaregistry.info/Elements/e/succeededByExpression.en> ;
    reg:name "succeededByExpression"@en ;
    reg:status <http://metadataregistry.org/uri/RegStatus/1001> ;
    a rdf:Property ;
    rdfs:domain <http://rdaregistry.info/Elements/c/C10006> ;
    rdfs:isDefinedBy <http://rdaregistry.info/Elements/e/> ;
    rdfs:label "is succeeded by (expression)"@en ;
    rdfs:subPropertyOf <http://rdaregistry.info/Elements/e/P20235> ;
    skos:definition "Relates an expression to an expression of a work that succeeds, that is, is later in time or after in a narrative, etc., a preceding expression."@en .

<http://rdaregistry.info/Elements/e/P20170>
    rdakit:instructionNumber "24.5" ;
    rdakit:toolkitDefinition "An expression of a work that systematically and comprehensively condenses a source expression."@en, "Expression d’une œuvre qui abrège de manière systématique et complète l’expression source."@fr, "Una expresión de una obra que sistemática e integralmente condensa la expresión fuente."@es ;
    rdakit:toolkitLabel "compendiada como (expresión)"@es, "condensé comme (expression)"@fr, "digested as (expression)"@en ;
    reg:hasSubproperty <http://rdaregistry.info/Elements/e/object/P20170> ;
    reg:hasUnconstrained <http://rdaregistry.info/Elements/u/P60279> ;
    reg:lexicalAlias <http://rdaregistry.info/Elements/e/digestedAsExpression.en> ;
    reg:name "digestedAsExpression"@en ;
    reg:status <http://metadataregistry.org/uri/RegStatus/1001> ;
    a rdf:Property ;
    rdfs:domain <http://rdaregistry.info/Elements/c/C10006> ;
    rdfs:isDefinedBy <http://rdaregistry.info/Elements/e/> ;
    rdfs:label "is digested as (expression)"@en ;
    rdfs:subPropertyOf <http://rdaregistry.info/Elements/e/P20203> ;
    skos:definition "Relates an expression to an expression of a work that systematically and comprehensively condenses a source expression."@en .

<http://rdaregistry.info/Elements/e/P20171>
    rdakit:instructionNumber "24.5" ;
    rdakit:toolkitDefinition "An expression of a work that translates the text of a source expression into a language different from that of an original work."@en, "Expression d’une œuvre qui traduit le texte de l’expression source dans une langue différente de celle de l’œuvre d’origine."@fr, "Una expresión de una obra que traduce el texto de una expresión fuente a una lengua diferente a la de la obra original."@es ;
    rdakit:toolkitLabel "traducida como"@es, "traduit comme"@fr, "translated as"@en ;
    reg:hasSubproperty <http://rdaregistry.info/Elements/e/P20079>, <http://rdaregistry.info/Elements/e/object/P20171> ;
    reg:hasUnconstrained <http://rdaregistry.info/Elements/u/P60280> ;
    reg:lexicalAlias <http://rdaregistry.info/Elements/e/translatedAs.en> ;
    reg:name "translatedAs"@en ;
    reg:status <http://metadataregistry.org/uri/RegStatus/1001> ;
    a rdf:Property ;
    rdfs:domain <http://rdaregistry.info/Elements/c/C10006> ;
    rdfs:isDefinedBy <http://rdaregistry.info/Elements/e/> ;
    rdfs:label "is translated as"@en ;
    rdfs:subPropertyOf <http://rdaregistry.info/Elements/e/P20203> ;
    skos:definition "Relates an expression to an expression of a work that translates the text of a source expression into a language different from that of an original work."@en .

<http://rdaregistry.info/Elements/e/P20172>
    rdakit:instructionNumber "24.5" ;
    rdakit:toolkitDefinition "An expression of a work that updates or otherwise complements a predominant expression."@en, "Expression d’une œuvre qui met à jour ou complète d’une autre façon l’expression prédominante."@fr, "Una expresión de una obra que actualiza o complementa la expresión principal."@es ;
    rdakit:toolkitLabel "suplemento (expresión)"@es, "supplement (expression)"@en, "supplément (expression)"@fr ;
    reg:hasSubproperty <http://rdaregistry.info/Elements/e/object/P20172> ;
    reg:hasUnconstrained <http://rdaregistry.info/Elements/u/P60281> ;
    reg:lexicalAlias <http://rdaregistry.info/Elements/e/supplementExpression.en> ;
    reg:name "supplementExpression"@en ;
    reg:status <http://metadataregistry.org/uri/RegStatus/1001> ;
    a rdf:Property ;
    rdfs:domain <http://rdaregistry.info/Elements/c/C10006> ;
    rdfs:isDefinedBy <http://rdaregistry.info/Elements/e/> ;
    rdfs:label "is supplement (expression)"@en ;
    rdfs:subPropertyOf <http://rdaregistry.info/Elements/e/P20105> ;
    skos:definition "Relates an expression to an expression of a work that updates or otherwise complements a predominant expression."@en .

<http://rdaregistry.info/Elements/e/P20173>
    rdakit:instructionNumber "24.5" ;
    rdakit:toolkitDefinition "An expression of a work that uses the text as a screenplay for a motion picture."@en, "Expression d’une œuvre qui utilise le texte comme scénario d’un film."@fr, "Una expresión de una obra que utiliza el texto como un guión para una película cinematográfica."@es ;
    rdakit:toolkitLabel "guión para la película cinematográfica (expresión)"@es, "screenplay for motion picture (expression)"@en, "scénario pour le film (expression)"@fr ;
    reg:hasSubproperty <http://rdaregistry.info/Elements/e/object/P20173> ;
    reg:hasUnconstrained <http://rdaregistry.info/Elements/u/P60282> ;
    reg:lexicalAlias <http://rdaregistry.info/Elements/e/screenplayForMotionPictureExpression.en> ;
    reg:name "screenplayForMotionPictureExpression"@en ;
    reg:status <http://metadataregistry.org/uri/RegStatus/1001> ;
    a rdf:Property ;
    rdfs:domain <http://rdaregistry.info/Elements/c/C10006> ;
    rdfs:isDefinedBy <http://rdaregistry.info/Elements/e/> ;
    rdfs:label "is screenplay for motion picture (expression)"@en ;
    rdfs:subPropertyOf <http://rdaregistry.info/Elements/e/P20102> ;
    skos:definition "Relates an expression to an expression of a work that uses the text as a screenplay for a motion picture."@en .

<http://rdaregistry.info/Elements/e/P20174>
    rdakit:instructionNumber "24.5" ;
    rdakit:toolkitDefinition "An expression of a work that uses the text as a screenplay for a television program."@en, "Expression d’une œuvre qui utilise le texte comme scénario d’une émission de télévision."@fr, "Una expresión de una obra que utiliza el texto como un guión para un programa de televisión."@es ;
    rdakit:toolkitLabel "guión para el programa de televisión (expresión)"@es, "screenplay for television program (expression)"@en, "scénario pour l’émission de télévision (expression)"@fr ;
    reg:hasSubproperty <http://rdaregistry.info/Elements/e/object/P20174> ;
    reg:hasUnconstrained <http://rdaregistry.info/Elements/u/P60283> ;
    reg:lexicalAlias <http://rdaregistry.info/Elements/e/screenplayForTelevisionProgramExpression.en> ;
    reg:name "screenplayForTelevisionProgramExpression"@en ;
    reg:status <http://metadataregistry.org/uri/RegStatus/1001> ;
    a rdf:Property ;
    rdfs:domain <http://rdaregistry.info/Elements/c/C10006> ;
    rdfs:isDefinedBy <http://rdaregistry.info/Elements/e/> ;
    rdfs:label "is screenplay for television program (expression)"@en ;
    rdfs:subPropertyOf <http://rdaregistry.info/Elements/e/P20102> ;
    skos:definition "Relates an expression to an expression of a work that uses the text as a screenplay for a television program."@en .

<http://rdaregistry.info/Elements/e/P20175>
    rdakit:instructionNumber "24.5" ;
    rdakit:toolkitDefinition "An expression of a work that uses the text as a screenplay for a video."@en, "Expression d’une œuvre qui utilise le texte comme scénario d’une vidéo."@fr, "Una expresión de una obra que utiliza el texto como un guión para un video."@es ;
    rdakit:toolkitLabel "guión para el video (expresión)"@es, "screenplay for video (expression)"@en, "scénario pour la vidéo (expression)"@fr ;
    reg:hasSubproperty <http://rdaregistry.info/Elements/e/object/P20175> ;
    reg:hasUnconstrained <http://rdaregistry.info/Elements/u/P60284> ;
    reg:lexicalAlias <http://rdaregistry.info/Elements/e/screenplayForVideoExpression.en> ;
    reg:name "screenplayForVideoExpression"@en ;
    reg:status <http://metadataregistry.org/uri/RegStatus/1001> ;
    a rdf:Property ;
    rdfs:domain <http://rdaregistry.info/Elements/c/C10006> ;
    rdfs:isDefinedBy <http://rdaregistry.info/Elements/e/> ;
    rdfs:label "is screenplay for video (expression)"@en ;
    rdfs:subPropertyOf <http://rdaregistry.info/Elements/e/P20102> ;
    skos:definition "Relates an expression to an expression of a work that uses the text as a screenplay for a video."@en .

<http://rdaregistry.info/Elements/e/P20176>
    rdakit:instructionNumber "24.5" ;
    rdakit:toolkitDefinition "An expression of a work that uses the text as a script for a radio program."@en, "Expression d’une œuvre qui utilise le texte de l’œuvre source comme script d’une émission de radio."@fr, "Una expresión de una obra que utiliza el texto de la obra fuente como el guión para un programa radiofónico."@es ;
    rdakit:toolkitLabel "guión para el programa de radio (expresión)"@es, "script for radio program (expression)"@en, "script pour l’émission de radio (expression)"@fr ;
    reg:hasSubproperty <http://rdaregistry.info/Elements/e/object/P20176> ;
    reg:hasUnconstrained <http://rdaregistry.info/Elements/u/P60285> ;
    reg:lexicalAlias <http://rdaregistry.info/Elements/e/scriptForRadioProgramExpression.en> ;
    reg:name "scriptForRadioProgramExpression"@en ;
    reg:status <http://metadataregistry.org/uri/RegStatus/1001> ;
    a rdf:Property ;
    rdfs:domain <http://rdaregistry.info/Elements/c/C10006> ;
    rdfs:isDefinedBy <http://rdaregistry.info/Elements/e/> ;
    rdfs:label "is script for radio program (expression)"@en ;
    rdfs:subPropertyOf <http://rdaregistry.info/Elements/e/P20100> ;
    skos:definition "Relates an expression to an expression of a work that uses the text as a script for a radio program."@en .

<http://rdaregistry.info/Elements/e/P20177>
    rdakit:instructionNumber "24.5" ;
    rdakit:toolkitDefinition "An expression of a work whose content is completed with brief content from an expression of another work."@en, "Expression d’une œuvre à laquelle sont ajoutées de brèves informations additionnelles, moins étendues qu’un supplément, mais essentielles à la complétude du contenu de l’œuvre ; ces informations sont généralement ajoutées à la fin du contenu, mais peuvent aussi parfois être publiées séparément."@fr, "Una expresión de una obra a la cual es añadido material adicional, menos extenso que un suplemento, pero esencial para la integridad del contenido de la obra; es añadido generalmente al final del contenido pero algunas veces se publica separadamente."@es ;
    rdakit:toolkitLabel "addenda de (expression)"@fr, "addenda to (expression)"@en, "adenda de (expresión)"@es ;
    reg:hasSubproperty <http://rdaregistry.info/Elements/e/object/P20177> ;
    reg:hasUnconstrained <http://rdaregistry.info/Elements/u/P60286> ;
    reg:lexicalAlias <http://rdaregistry.info/Elements/e/addendaToExpression.en> ;
    reg:name "addendaToExpression"@en ;
    reg:status <http://metadataregistry.org/uri/RegStatus/1001> ;
    a rdf:Property ;
    rdfs:domain <http://rdaregistry.info/Elements/c/C10006> ;
    rdfs:isDefinedBy <http://rdaregistry.info/Elements/e/> ;
    rdfs:label "is addenda to (expression)"@en ;
    rdfs:subPropertyOf <http://rdaregistry.info/Elements/e/P20192> ;
    skos:definition "Relates an expression to an expression of a work whose content is completed with brief content from an expression of another work."@en .

<http://rdaregistry.info/Elements/e/P20178>
    reg:status <http://metadataregistry.org/uri/RegStatus/1008> ;
    a rdf:Property ;
    rdfs:isDefinedBy <http://rdaregistry.info/Elements/e/> ;
    rdfs:subPropertyOf <http://rdaregistry.info/Elements/e/P20072> .

<http://rdaregistry.info/Elements/e/P20179>
    rdakit:instructionNumber "24.5" ;
    rdakit:toolkitDefinition "An expression of a work used as the basis for a brief recapitulation of its content."@en, "Expression d’une œuvre servant de base à une brève récapitulation de son contenu."@fr, "Una expresión de una obra usada como base para una recapitulación breve de su contenido."@es ;
    rdakit:toolkitLabel "résumé de (expression)"@fr, "sumario de (expresión)"@es, "summary of (expression)"@en ;
    reg:hasSubproperty <http://rdaregistry.info/Elements/e/object/P20179> ;
    reg:hasUnconstrained <http://rdaregistry.info/Elements/u/P60289> ;
    reg:lexicalAlias <http://rdaregistry.info/Elements/e/summaryOfExpression.en> ;
    reg:name "summaryOfExpression"@en ;
    reg:status <http://metadataregistry.org/uri/RegStatus/1001> ;
    a rdf:Property ;
    rdfs:domain <http://rdaregistry.info/Elements/c/C10006> ;
    rdfs:isDefinedBy <http://rdaregistry.info/Elements/e/> ;
    rdfs:label "is summary of (expression)"@en ;
    rdfs:subPropertyOf <http://rdaregistry.info/Elements/e/P20204> ;
    skos:definition "Relates an expression to an expression of a work used as the basis for a brief recapitulation of its content."@en .

<http://rdaregistry.info/Elements/e/P20180>
    rdakit:instructionNumber "24.5" ;
    rdakit:toolkitDefinition "An expression of a work used as the basis for a catalogue, i.e., a complete enumeration of items arranged systematically."@en, "Expression d’une œuvre servant de base à un catalogue, c’est-à-dire une énumération complète des items classés systématiquement."@fr, "Una expresión de una obra utilizada como base para un catálogo, i.e., una enumeración completa de ítems ordenados sistemáticamente."@es ;
    rdakit:toolkitLabel "catalogue de (expression)"@fr, "catalogue of (expression)"@en, "catálogo de (expresión)"@es ;
    reg:hasSubproperty <http://rdaregistry.info/Elements/e/object/P20180> ;
    reg:hasUnconstrained <http://rdaregistry.info/Elements/u/P60290> ;
    reg:lexicalAlias <http://rdaregistry.info/Elements/e/catalogueOfExpression.en> ;
    reg:name "catalogueOfExpression"@en ;
    reg:status <http://metadataregistry.org/uri/RegStatus/1001> ;
    a rdf:Property ;
    rdfs:domain <http://rdaregistry.info/Elements/c/C10006> ;
    rdfs:isDefinedBy <http://rdaregistry.info/Elements/e/> ;
    rdfs:label "is catalogue of (expression)"@en ;
    rdfs:subPropertyOf <http://rdaregistry.info/Elements/e/P20192> ;
    skos:definition "Relates an expression to an expression of a work used as the basis for a catalogue, i.e., a complete enumeration of items arranged systematically."@en .

<http://rdaregistry.info/Elements/e/P20181>
    rdakit:instructionNumber "24.5" ;
    rdakit:toolkitDefinition "An expression of a work used as the basis for a concordance, i.e., an index of all the words in a predominant expression."@en, "Expression d’une œuvre servant de base à une concordance, c’est-à-dire un index de tous les mots de l’expression prédominante."@fr, "Una expresión de una obra utilizada como base para una concordancia, i.e., un índice de todas las palabras en la expresión principal."@es ;
    rdakit:toolkitLabel "concordance de (expression)"@fr, "concordance to (expression)"@en, "concordancia de (expresión)"@es ;
    reg:hasSubproperty <http://rdaregistry.info/Elements/e/object/P20181> ;
    reg:hasUnconstrained <http://rdaregistry.info/Elements/u/P60291> ;
    reg:lexicalAlias <http://rdaregistry.info/Elements/e/concordanceToExpression.en> ;
    reg:name "concordanceToExpression"@en ;
    reg:status <http://metadataregistry.org/uri/RegStatus/1001> ;
    a rdf:Property ;
    rdfs:domain <http://rdaregistry.info/Elements/c/C10006> ;
    rdfs:isDefinedBy <http://rdaregistry.info/Elements/e/> ;
    rdfs:label "is concordance to (expression)"@en ;
    rdfs:subPropertyOf <http://rdaregistry.info/Elements/e/P20192> ;
    skos:definition "Relates an expression to an expression of a work used as the basis for a concordance, i.e., an index of all the words in a predominant expression."@en .

<http://rdaregistry.info/Elements/e/P20182>
    reg:status <http://metadataregistry.org/uri/RegStatus/1008> ;
    a rdf:Property ;
    rdfs:isDefinedBy <http://rdaregistry.info/Elements/e/> ;
    rdfs:subPropertyOf <http://rdaregistry.info/Elements/e/P20072> .

<http://rdaregistry.info/Elements/e/P20183>
    rdakit:instructionNumber "24.5" ;
    rdakit:toolkitDefinition "An expression of a work that has been adapted as a work consisting of movement."@en, "Expression d’une œuvre qui a été adaptée en œuvre consistant en mouvement (par exemple, de la danse)."@fr, "Una expresión de una obra que ha sido adaptada como una obra que consiste en movimiento (p. ej., danza)."@es ;
    rdakit:toolkitLabel "adaptación coreográfica de (expresión)"@es, "adaptation chorégraphique de (expression)"@fr, "choreographic adaptation of (expression)"@en ;
    reg:hasSubproperty <http://rdaregistry.info/Elements/e/object/P20183> ;
    reg:hasUnconstrained <http://rdaregistry.info/Elements/u/P60293> ;
    reg:lexicalAlias <http://rdaregistry.info/Elements/e/choreographicAdaptationOfExpression.en> ;
    reg:name "choreographicAdaptationOfExpression"@en ;
    reg:status <http://metadataregistry.org/uri/RegStatus/1001> ;
    a rdf:Property ;
    rdfs:domain <http://rdaregistry.info/Elements/c/C10006> ;
    rdfs:isDefinedBy <http://rdaregistry.info/Elements/e/> ;
    rdfs:label "is choreographic adaptation of (expression)"@en ;
    rdfs:subPropertyOf <http://rdaregistry.info/Elements/e/P20152> ;
    skos:definition "Relates an expression to an expression of a work that has been adapted as a work consisting of movement."@en .

<http://rdaregistry.info/Elements/e/P20184>
    rdakit:instructionNumber "24.5" ;
    rdakit:toolkitDefinition "An expression of a work used as the basis for a derivative work that enlarges upon the content of a source work."@en, "Expression d’une œuvre servant de base à une œuvre dérivée qui accroît le contenu de l’œuvre source."@fr, "Una expresión de una obra utilizada como base para una obra derivada que alarga el contenido de la obra fuente."@es ;
    rdakit:toolkitLabel "expanded version of (expression)"@en, "version augmentée de (expression)"@fr, "versión ampliada de (expresión)"@es ;
    reg:hasSubproperty <http://rdaregistry.info/Elements/e/object/P20184> ;
    reg:hasUnconstrained <http://rdaregistry.info/Elements/u/P60294> ;
    reg:lexicalAlias <http://rdaregistry.info/Elements/e/expandedVersionOfExpression.en> ;
    reg:name "expandedVersionOfExpression"@en ;
    reg:status <http://metadataregistry.org/uri/RegStatus/1001> ;
    a rdf:Property ;
    rdfs:domain <http://rdaregistry.info/Elements/c/C10006> ;
    rdfs:isDefinedBy <http://rdaregistry.info/Elements/e/> ;
    rdfs:label "is expanded version of (expression)"@en ;
    rdfs:subPropertyOf <http://rdaregistry.info/Elements/e/P20204> ;
    skos:definition "Relates an expression to an expression of a work used as the basis for a derivative work that enlarges upon the content of a source work."@en .

<http://rdaregistry.info/Elements/e/P20185>
    rdakit:instructionNumber "24.5" ;
    rdakit:toolkitDefinition "An expression of a work used as a basis for a new motion picture, radio program, television program, or video."@en, "Expression d’une œuvre servant de base à un nouveau film, une nouvelle émission de radio, une nouvelle émission de télévision ou une nouvelle vidéo."@fr, "Una expresión de una obra utilizada como base para una nueva película cinematográfica, programa de radio, televisión o video."@es ;
    rdakit:toolkitLabel "nouvelle version de (expression)"@fr, "remake de (expresión)"@es, "remake of (expression)"@en ;
    reg:hasSubproperty <http://rdaregistry.info/Elements/e/object/P20185> ;
    reg:hasUnconstrained <http://rdaregistry.info/Elements/u/P60295> ;
    reg:lexicalAlias <http://rdaregistry.info/Elements/e/remakeOfExpression.en> ;
    reg:name "remakeOfExpression"@en ;
    reg:status <http://metadataregistry.org/uri/RegStatus/1001> ;
    a rdf:Property ;
    rdfs:domain <http://rdaregistry.info/Elements/c/C10006> ;
    rdfs:isDefinedBy <http://rdaregistry.info/Elements/e/> ;
    rdfs:label "is remake of (expression)"@en ;
    rdfs:subPropertyOf <http://rdaregistry.info/Elements/e/P20204> ;
    skos:definition "Relates an expression to an expression of a work used as a basis for a new motion picture, radio program, television program, or video."@en .

<http://rdaregistry.info/Elements/e/P20186>
    rdakit:instructionNumber "24.5" ;
    rdakit:toolkitDefinition "An expression of a work used as the basis for a paraphrase, i.e., a restating of the content of a source work in a different form."@en, "Expression d’une œuvre servant de base à une paraphrase, c’est-à-dire une reprise du contenu de l’œuvre source sous une formulation différente."@fr, "Una expresión de una obra utilizada como base para una paráfrasis, i. e., replanteamiento del contenido de la obra fuente en una forma diferente."@es ;
    rdakit:toolkitLabel "paraphrase de (expression)"@fr, "paraphrase of (expression)"@en, "paráfrasis de (expresión)"@es ;
    reg:hasSubproperty <http://rdaregistry.info/Elements/e/object/P20186> ;
    reg:hasUnconstrained <http://rdaregistry.info/Elements/u/P60296> ;
    reg:lexicalAlias <http://rdaregistry.info/Elements/e/paraphraseOfExpression.en> ;
    reg:name "paraphraseOfExpression"@en ;
    reg:status <http://metadataregistry.org/uri/RegStatus/1001> ;
    a rdf:Property ;
    rdfs:domain <http://rdaregistry.info/Elements/c/C10006> ;
    rdfs:isDefinedBy <http://rdaregistry.info/Elements/e/> ;
    rdfs:label "is paraphrase of (expression)"@en ;
    rdfs:subPropertyOf <http://rdaregistry.info/Elements/e/P20204> ;
    skos:definition "Relates an expression to an expression of a work used as the basis for a paraphrase, i.e., a restating of the content of a source work in a different form."@en .

<http://rdaregistry.info/Elements/e/P20187>
    reg:status <http://metadataregistry.org/uri/RegStatus/1008> ;
    a rdf:Property ;
    rdfs:isDefinedBy <http://rdaregistry.info/Elements/e/> ;
    rdfs:subPropertyOf <http://rdaregistry.info/Elements/e/P20072> .

<http://rdaregistry.info/Elements/e/P20188>
    rdakit:instructionNumber "24.5" ;
    rdakit:toolkitDefinition "An expression of a work used as the basis for an index, i.e., a systematic, alphabetical guide to the contents of a predominant expression, usually keyed to page numbers or other reference codes."@en, "Expression d’une œuvre servant de base à un index, c’est-à-dire un guide méthodique et alphabétique du contenu de l’expression prédominante, renvoyant généralement à des numéros de page ou à d’autres codes de référence."@fr, "Una expresión de una obra utilizada como base para un índice, i.e., una guía alfabética y sistemática del contenido la entidad principal, generalmente indicando los números de página u otros códigos de referencia."@es ;
    rdakit:toolkitLabel "index de (expression)"@fr, "index to (expression)"@en, "índice de (expresión)"@es ;
    reg:hasSubproperty <http://rdaregistry.info/Elements/e/object/P20188> ;
    reg:hasUnconstrained <http://rdaregistry.info/Elements/u/P60302> ;
    reg:lexicalAlias <http://rdaregistry.info/Elements/e/indexToExpression.en> ;
    reg:name "indexToExpression"@en ;
    reg:status <http://metadataregistry.org/uri/RegStatus/1001> ;
    a rdf:Property ;
    rdfs:domain <http://rdaregistry.info/Elements/c/C10006> ;
    rdfs:isDefinedBy <http://rdaregistry.info/Elements/e/> ;
    rdfs:label "is index to (expression)"@en ;
    rdfs:subPropertyOf <http://rdaregistry.info/Elements/e/P20192> ;
    skos:definition "Relates an expression to an expression of a work used as the basis for an index, i.e., a systematic, alphabetical guide to the contents of a predominant expression, usually keyed to page numbers or other reference codes."@en .

<http://rdaregistry.info/Elements/e/P20189>
    rdakit:instructionNumber "24.5" ;
    rdakit:toolkitDefinition "An expression of a work used as the basis for an updated, corrected, or expanded version."@en, "Expression d’une œuvre servant de base à une version mise à jour, corrigée ou augmentée."@fr, "Una expresión de una obra utilizada como base para una versión actualizada, corregida o ampliada."@es ;
    rdakit:toolkitLabel "revision of"@en, "revisión de"@es, "révision de"@fr ;
    reg:hasSubproperty <http://rdaregistry.info/Elements/e/object/P20189> ;
    reg:hasUnconstrained <http://rdaregistry.info/Elements/u/P60303> ;
    reg:lexicalAlias <http://rdaregistry.info/Elements/e/revisionOf.en> ;
    reg:name "revisionOf"@en ;
    reg:status <http://metadataregistry.org/uri/RegStatus/1001> ;
    a rdf:Property ;
    rdfs:domain <http://rdaregistry.info/Elements/c/C10006> ;
    rdfs:isDefinedBy <http://rdaregistry.info/Elements/e/> ;
    rdfs:label "is revision of"@en ;
    rdfs:subPropertyOf <http://rdaregistry.info/Elements/e/P20204> ;
    skos:definition "Relates an expression to an expression of a work used as the basis for an updated, corrected, or expanded version."@en .

<http://rdaregistry.info/Elements/e/P20190>
    rdakit:instructionNumber "24.5" ;
    rdakit:toolkitDefinition "An expression of a work used as the basis for the text of an opera or other work for the musical stage, or an oratorio."@en, "Expression d’une œuvre servant de base au texte d’un opéra ou d’une autre œuvre pour la scène musicale, ou bien d’un oratorio."@fr, "Una expresión de una obra usada como base para el texto de una ópera u otra obra para representación musical u oratorio."@es ;
    rdakit:toolkitLabel "libreto basado en (expresión)"@es, "libretto based on (expression)"@en, "livret basé sur (expression)"@fr ;
    reg:hasSubproperty <http://rdaregistry.info/Elements/e/object/P20190> ;
    reg:hasUnconstrained <http://rdaregistry.info/Elements/u/P60304> ;
    reg:lexicalAlias <http://rdaregistry.info/Elements/e/librettoBasedOnExpression.en> ;
    reg:name "librettoBasedOnExpression"@en ;
    reg:status <http://metadataregistry.org/uri/RegStatus/1001> ;
    a rdf:Property ;
    rdfs:domain <http://rdaregistry.info/Elements/c/C10006> ;
    rdfs:isDefinedBy <http://rdaregistry.info/Elements/e/> ;
    rdfs:label "is libretto based on (expression)"@en ;
    rdfs:subPropertyOf <http://rdaregistry.info/Elements/e/P20152> ;
    skos:definition "Relates an expression to an expression of a work that has been adapted as the text of an opera or other work for the musical stage, or an oratorio."@en .

<http://rdaregistry.info/Elements/e/P20191>
    rdakit:instructionNumber "24.5" ;
    rdakit:toolkitDefinition "An expression of a work whose content continues an expression of an earlier work."@en, "Expression d’une œuvre dont le contenu continue une expression d’une œuvre antérieure."@fr, "Una expresión de una obra cuyo contenido continúa una entidad anterior bajo un título nuevo."@es ;
    rdakit:toolkitLabel "continuada por (expresión)"@es, "continued by (expression)"@en, "continué par (expression)"@fr ;
    reg:hasSubproperty <http://rdaregistry.info/Elements/e/object/P20191> ;
    reg:hasUnconstrained <http://rdaregistry.info/Elements/u/P60306> ;
    reg:lexicalAlias <http://rdaregistry.info/Elements/e/continuedByExpression.en> ;
    reg:name "continuedByExpression"@en ;
    reg:status <http://metadataregistry.org/uri/RegStatus/1001> ;
    a rdf:Property ;
    rdfs:domain <http://rdaregistry.info/Elements/c/C10006> ;
    rdfs:isDefinedBy <http://rdaregistry.info/Elements/e/> ;
    rdfs:label "is continued by (expression)"@en ;
    rdfs:subPropertyOf <http://rdaregistry.info/Elements/e/P20169> ;
    skos:definition "Relates an expression to an expression of a work whose content continues an expression of an earlier work."@en ;
    skos:scopeNote "This relationship applies generally to serials."@en .

<http://rdaregistry.info/Elements/e/P20192>
    rdakit:instructionNumber "24.5" ;
    rdakit:toolkitDefinition "An expression of a work whose content is added to by another expression."@en, "Expression d’une œuvre dont le contenu est accru par une autre expression."@fr, "Una expresión de una obra cuyo contenido es añadido por otra expresión."@es ;
    rdakit:toolkitLabel "augmentation de (expression)"@fr, "augmentation of (expression)"@en, "aumento de (expresión)"@es ;
    reg:hasSubproperty <http://rdaregistry.info/Elements/e/P20083>, <http://rdaregistry.info/Elements/e/P20089>, <http://rdaregistry.info/Elements/e/P20146>, <http://rdaregistry.info/Elements/e/P20147>, <http://rdaregistry.info/Elements/e/P20148>, <http://rdaregistry.info/Elements/e/P20151>, <http://rdaregistry.info/Elements/e/P20177>, <http://rdaregistry.info/Elements/e/P20180>, <http://rdaregistry.info/Elements/e/P20181>, <http://rdaregistry.info/Elements/e/P20188>, <http://rdaregistry.info/Elements/e/P20197>, <http://rdaregistry.info/Elements/e/object/P20192> ;
    reg:hasUnconstrained <http://rdaregistry.info/Elements/u/P60307> ;
    reg:lexicalAlias <http://rdaregistry.info/Elements/e/augmentationOfExpression.en> ;
    reg:name "augmentationOfExpression"@en ;
    reg:status <http://metadataregistry.org/uri/RegStatus/1001> ;
    a rdf:Property ;
    rdfs:domain <http://rdaregistry.info/Elements/c/C10006> ;
    rdfs:isDefinedBy <http://rdaregistry.info/Elements/e/> ;
    rdfs:label "is augmentation of (expression)"@en ;
    rdfs:subPropertyOf <http://rdaregistry.info/Elements/e/P20232> ;
    skos:definition "Relates an expression to an expression of a work whose content is added to by another expression."@en .

<http://rdaregistry.info/Elements/e/P20193>
    rdakit:instructionNumber "24.5" ;
    rdakit:toolkitDefinition "An expression of a work whose contents have been abstracted by an abstracting and indexing service."@en, "Expression d’une œuvre dont le contenu a été résumé par un service d’analyse et d’indexation."@fr, "Una expresión de una obra cuyos contenidos han sido resumidos por un servicio de indización y resúmenes."@es ;
    rdakit:toolkitLabel "abstracts for (expression)"@en, "resúmenes de (expresión)"@es, "résumés analytiques pour (expression)"@fr ;
    reg:hasSubproperty <http://rdaregistry.info/Elements/e/object/P20193> ;
    reg:hasUnconstrained <http://rdaregistry.info/Elements/u/P60308> ;
    reg:lexicalAlias <http://rdaregistry.info/Elements/e/abstractsForExpression.en> ;
    reg:name "abstractsForExpression"@en ;
    reg:status <http://metadataregistry.org/uri/RegStatus/1001> ;
    a rdf:Property ;
    rdfs:domain <http://rdaregistry.info/Elements/c/C10006> ;
    rdfs:isDefinedBy <http://rdaregistry.info/Elements/e/> ;
    rdfs:label "is abstracts for (expression)"@en ;
    rdfs:subPropertyOf <http://rdaregistry.info/Elements/e/P20204> ;
    skos:definition "Relates an expression to an expression of a work whose contents have been abstracted by an abstracting and indexing service."@en .

<http://rdaregistry.info/Elements/e/P20194>
    rdakit:instructionNumber "24.5" ;
    rdakit:toolkitDefinition "An expression of a work whose contents have been indexed by an abstracting and indexing service."@en, "Expression d’une œuvre dont le contenu a été indexé par un service d’analyse et d’indexation."@fr, "Una expresión de una obra cuyo contenido ha sido indizado por un servicio de indización y resúmenes."@es ;
    rdakit:toolkitLabel "indexation pour (expression)"@fr, "indexing for (expression)"@en, "indización de (expresión)"@es ;
    reg:hasSubproperty <http://rdaregistry.info/Elements/e/object/P20194> ;
    reg:hasUnconstrained <http://rdaregistry.info/Elements/u/P60309> ;
    reg:lexicalAlias <http://rdaregistry.info/Elements/e/indexingForExpression.en> ;
    reg:name "indexingForExpression"@en ;
    reg:status <http://metadataregistry.org/uri/RegStatus/1001> ;
    a rdf:Property ;
    rdfs:domain <http://rdaregistry.info/Elements/c/C10006> ;
    rdfs:isDefinedBy <http://rdaregistry.info/Elements/e/> ;
    rdfs:label "is indexing for (expression)"@en ;
    rdfs:subPropertyOf <http://rdaregistry.info/Elements/e/P20204> ;
    skos:definition "Relates an expression to an expression of a work whose contents have been indexed by an abstracting and indexing service."@en .

<http://rdaregistry.info/Elements/e/P20195>
    rdakit:instructionNumber "24.5" ;
    rdakit:toolkitDefinition "An expression of a work whose style or content is copied in a derivative work."@en, "Expression d’une œuvre dont le style ou le contenu est copié dans une œuvre dérivée."@fr, "Una expresión de una obra cuyo estilo o contenido es copiado en una obra derivada."@es ;
    rdakit:toolkitLabel "imitación de (expresión)"@es, "imitation de (expression)"@fr, "imitation of (expression)"@en ;
    reg:hasSubproperty <http://rdaregistry.info/Elements/e/P20196>, <http://rdaregistry.info/Elements/e/object/P20195> ;
    reg:hasUnconstrained <http://rdaregistry.info/Elements/u/P60311> ;
    reg:lexicalAlias <http://rdaregistry.info/Elements/e/imitationOfExpression.en> ;
    reg:name "imitationOfExpression"@en ;
    reg:status <http://metadataregistry.org/uri/RegStatus/1001> ;
    a rdf:Property ;
    rdfs:domain <http://rdaregistry.info/Elements/c/C10006> ;
    rdfs:isDefinedBy <http://rdaregistry.info/Elements/e/> ;
    rdfs:label "is imitation of (expression)"@en ;
    rdfs:subPropertyOf <http://rdaregistry.info/Elements/e/P20204> ;
    skos:definition "Relates an expression to an expression of a work whose style or content is copied in a derivative work."@en .

<http://rdaregistry.info/Elements/e/P20196>
    rdakit:instructionNumber "24.5" ;
    rdakit:toolkitDefinition "An expression of a work whose style or content is imitated for comic effect."@en, "Expression d’une œuvre dont le style ou le contenu est imité dans le but de produire un effet comique."@fr, "Una expresión de una obra cuyo estilo o contenido es imitado para crear un efecto cómico."@es ;
    rdakit:toolkitLabel "parodia de (expresión)"@es, "parodie de (expression)"@fr, "parody of (expression)"@en ;
    reg:hasSubproperty <http://rdaregistry.info/Elements/e/object/P20196> ;
    reg:hasUnconstrained <http://rdaregistry.info/Elements/u/P60312> ;
    reg:lexicalAlias <http://rdaregistry.info/Elements/e/parodyOfExpression.en> ;
    reg:name "parodyOfExpression"@en ;
    reg:status <http://metadataregistry.org/uri/RegStatus/1001> ;
    a rdf:Property ;
    rdfs:domain <http://rdaregistry.info/Elements/c/C10006> ;
    rdfs:isDefinedBy <http://rdaregistry.info/Elements/e/> ;
    rdfs:label "is parody of (expression)"@en ;
    rdfs:subPropertyOf <http://rdaregistry.info/Elements/e/P20195> ;
    skos:definition "Relates an expression to an expression of a work whose style or content is imitated for comic effect."@en .

<http://rdaregistry.info/Elements/e/P20197>
    rdakit:instructionNumber "24.5" ;
    rdakit:toolkitDefinition "An expression of an archival collection that is described in a finding aid, i.e., a guide to the organization, arrangement, and contents of the collection."@en, "Expression d’une collection ou d’un fonds d’archives qui est décrit dans un instrument de recherche, c’est-à-dire un guide de l’organisation, du classement et du contenu de la collection ou du fonds."@fr, "Una expresión de una colección archivística que está descrita en una guía de búsqueda, i.e., una guía para la organización, ordenación y contenido de la colección."@es ;
    rdakit:toolkitLabel "finding aid for (expression)"@en, "guía de búsqueda de (expresión)"@es, "instrument de recherche pour (expression)"@fr ;
    reg:hasSubproperty <http://rdaregistry.info/Elements/e/object/P20197> ;
    reg:hasUnconstrained <http://rdaregistry.info/Elements/u/P60474> ;
    reg:lexicalAlias <http://rdaregistry.info/Elements/e/findingAidForExpression.en> ;
    reg:name "findingAidForExpression"@en ;
    reg:status <http://metadataregistry.org/uri/RegStatus/1001> ;
    a rdf:Property ;
    rdfs:domain <http://rdaregistry.info/Elements/c/C10006> ;
    rdfs:isDefinedBy <http://rdaregistry.info/Elements/e/> ;
    rdfs:label "is finding aid for (expression)"@en ;
    rdfs:subPropertyOf <http://rdaregistry.info/Elements/e/P20192> ;
    skos:definition "Relates an expression to an expression of an archival collection that is described in a finding aid, i.e., a guide to the organization, arrangement, and contents of the collection."@en .

<http://rdaregistry.info/Elements/e/P20198>
    rdakit:instructionNumber "24.5" ;
    rdakit:toolkitDefinition "An expression of an earlier work whose content has been partially replaced by a later expression, usually because the later work contains updated or new information that makes the earlier expression obsolete."@en, "Expression d’une œuvre antérieure dont le contenu a été partiellement remplacé par une expression ultérieure, généralement parce que l’œuvre ultérieure contient de l’information nouvelle ou mise à jour qui rend l’expression antérieure obsolète."@fr, "Una expresión de una obra anterior cuyo contenido ha sido reemplazado parcialmente por una expresión posterior, generalmente porque la obra posterior contiene información actualizada o nueva que hace obsoleta la expresión anterior."@es ;
    rdakit:toolkitLabel "reemplazo en parte de (expresión)"@es, "remplacement partiel de (expression)"@fr, "replacement in part of (expression)"@en ;
    reg:hasSubproperty <http://rdaregistry.info/Elements/e/object/P20198> ;
    reg:hasUnconstrained <http://rdaregistry.info/Elements/u/P60479> ;
    reg:lexicalAlias <http://rdaregistry.info/Elements/e/replacementInPartOfExpression.en> ;
    reg:name "replacementInPartOfExpression"@en ;
    reg:status <http://metadataregistry.org/uri/RegStatus/1001> ;
    a rdf:Property ;
    rdfs:domain <http://rdaregistry.info/Elements/c/C10006> ;
    rdfs:isDefinedBy <http://rdaregistry.info/Elements/e/> ;
    rdfs:label "is replacement in part of (expression)"@en ;
    rdfs:subPropertyOf <http://rdaregistry.info/Elements/e/P20154> ;
    skos:definition "Relates an expression to an expression of an earlier work whose content has been partially replaced by a later expression, usually because the later work contains updated or new information that makes the earlier expression obsolete."@en ;
    skos:scopeNote "This relationship applies generally to single-part units, multipart monographs, and integrating resources."@en .

<http://rdaregistry.info/Elements/e/P20199>
    rdakit:instructionNumber "24.5" ;
    rdakit:toolkitDefinition "An expression of an earlier work whose content has been replaced by a later expression, usually because the later work contains updated or new information that makes the earlier expression obsolete."@en, "Expression d’une œuvre antérieure dont le contenu a été remplacé par une expression ultérieure, généralement parce que l’œuvre ultérieure contient de l’information nouvelle ou mise à jour qui rend l’expression antérieure obsolète."@fr, "Una expresión de una obra anterior cuyo contenido ha sido reemplazado por una expresión posterior, generalmente porque la obra posterior contiene información actualizada o nueva que hace obsoleta la expresión anterior."@es ;
    rdakit:toolkitLabel "reemplazo de (expresión)"@es, "remplacement de (expression)"@fr, "replacement of (expression)"@en ;
    reg:hasSubproperty <http://rdaregistry.info/Elements/e/object/P20199> ;
    reg:hasUnconstrained <http://rdaregistry.info/Elements/u/P60480> ;
    reg:lexicalAlias <http://rdaregistry.info/Elements/e/replacementOfExpression.en> ;
    reg:name "replacementOfExpression"@en ;
    reg:status <http://metadataregistry.org/uri/RegStatus/1001> ;
    a rdf:Property ;
    rdfs:domain <http://rdaregistry.info/Elements/c/C10006> ;
    rdfs:isDefinedBy <http://rdaregistry.info/Elements/e/> ;
    rdfs:label "is replacement of (expression)"@en ;
    rdfs:subPropertyOf <http://rdaregistry.info/Elements/e/P20154> ;
    skos:definition "Relates an expression to an expression of an earlier work whose content has been replaced by a later expression, usually because the later work contains updated or new information that makes the earlier expression obsolete."@en ;
    skos:scopeNote "This relationship applies generally to single-part units, multipart monographs, and integrating resources."@en .

<http://rdaregistry.info/Elements/e/P20200>
    rdakit:instructionNumber "24.5" ;
    rdakit:toolkitDefinition "An expression of one of two or more works resulting from division of an earlier expression into separate expressions."@en, "Expression de l’une de deux ou plusieurs œuvres résultant de la division d’une expression antérieure en expressions séparées."@fr, "Una expresión de una de dos o más obras que resulta de la división de una entidad anterior en entidades separadas."@es ;
    rdakit:toolkitLabel "escindida en (expresión)"@es, "scindé en (expression)"@fr, "split into (expression)"@en ;
    reg:hasSubproperty <http://rdaregistry.info/Elements/e/object/P20200> ;
    reg:hasUnconstrained <http://rdaregistry.info/Elements/u/P60503> ;
    reg:lexicalAlias <http://rdaregistry.info/Elements/e/splitIntoExpression.en> ;
    reg:name "splitIntoExpression"@en ;
    reg:status <http://metadataregistry.org/uri/RegStatus/1001> ;
    a rdf:Property ;
    rdfs:domain <http://rdaregistry.info/Elements/c/C10006> ;
    rdfs:isDefinedBy <http://rdaregistry.info/Elements/e/> ;
    rdfs:label "is split into (expression)"@en ;
    rdfs:subPropertyOf <http://rdaregistry.info/Elements/e/P20169> ;
    skos:definition "Relates an expression to an expression of one of two or more works resulting from division of an earlier expression into separate expressions."@en .

<http://rdaregistry.info/Elements/e/P20201>
    rdakit:instructionNumber "24.5" ;
    rdakit:toolkitDefinition "An expression of a work that came together with one or more other expressions to form a new expression."@en, "Expression d’une œuvre qui s’est assemblée avec une ou plusieurs autres expressions pour former la nouvelle expression."@fr, "Una expresión de una obra que se une con una o más expresiones para formar una expresión nueva."@es ;
    rdakit:toolkitLabel "fusion de (expression)"@fr, "fusión de (expresión)"@es, "merger of (expression)"@en ;
    reg:hasSubproperty <http://rdaregistry.info/Elements/e/object/P20201> ;
    reg:hasUnconstrained <http://rdaregistry.info/Elements/u/P60505> ;
    reg:lexicalAlias <http://rdaregistry.info/Elements/e/mergerOfExpression.en> ;
    reg:name "mergerOfExpression"@en ;
    reg:status <http://metadataregistry.org/uri/RegStatus/1001> ;
    a rdf:Property ;
    rdfs:domain <http://rdaregistry.info/Elements/c/C10006> ;
    rdfs:isDefinedBy <http://rdaregistry.info/Elements/e/> ;
    rdfs:label "is merger of (expression)"@en ;
    rdfs:subPropertyOf <http://rdaregistry.info/Elements/e/P20154> ;
    skos:definition "Relates an expression to an expression of a work that came together with one or more other expressions to form a new expression."@en .

<http://rdaregistry.info/Elements/e/P20202>
    reg:hasSubproperty <http://rdaregistry.info/Elements/e/P20111>, <http://rdaregistry.info/Elements/e/P20112>, <http://rdaregistry.info/Elements/e/P20113>, <http://rdaregistry.info/Elements/e/P20116>, <http://rdaregistry.info/Elements/e/P20117> ;
    reg:status <http://metadataregistry.org/uri/RegStatus/1008> ;
    a rdf:Property ;
    rdfs:isDefinedBy <http://rdaregistry.info/Elements/e/> ;
    rdfs:subPropertyOf <http://rdaregistry.info/Elements/e/P20234> .

<http://rdaregistry.info/Elements/e/P20203>
    rdakit:instructionNumber "24.5" ;
    rdakit:toolkitDefinition "An expression that is a modification of a source expression."@en, "Expression qui est une modification d’une expression source."@fr, "Una expresión que es una modificación de una expresión fuente."@es ;
    rdakit:toolkitLabel "derivative (expression)"@en, "dérivé (expression)"@fr, "expresión derivada"@es ;
    reg:hasSubproperty <http://rdaregistry.info/Elements/e/P20082>, <http://rdaregistry.info/Elements/e/P20086>, <http://rdaregistry.info/Elements/e/P20087>, <http://rdaregistry.info/Elements/e/P20090>, <http://rdaregistry.info/Elements/e/P20091>, <http://rdaregistry.info/Elements/e/P20092>, <http://rdaregistry.info/Elements/e/P20104>, <http://rdaregistry.info/Elements/e/P20106>, <http://rdaregistry.info/Elements/e/P20110>, <http://rdaregistry.info/Elements/e/P20114>, <http://rdaregistry.info/Elements/e/P20115>, <http://rdaregistry.info/Elements/e/P20119>, <http://rdaregistry.info/Elements/e/P20153>, <http://rdaregistry.info/Elements/e/P20164>, <http://rdaregistry.info/Elements/e/P20165>, <http://rdaregistry.info/Elements/e/P20166>, <http://rdaregistry.info/Elements/e/P20170>, <http://rdaregistry.info/Elements/e/P20171>, <http://rdaregistry.info/Elements/e/P20204>, <http://rdaregistry.info/Elements/e/P20211>, <http://rdaregistry.info/Elements/e/object/P20203> ;
    reg:hasUnconstrained <http://rdaregistry.info/Elements/u/P60250> ;
    reg:lexicalAlias <http://rdaregistry.info/Elements/e/derivativeExpression.en> ;
    reg:name "derivativeExpression"@en ;
    reg:status <http://metadataregistry.org/uri/RegStatus/1001> ;
    a rdf:Property ;
    rdfs:domain <http://rdaregistry.info/Elements/c/C10006> ;
    rdfs:isDefinedBy <http://rdaregistry.info/Elements/e/> ;
    rdfs:label "is derivative (expression)"@en ;
    rdfs:subPropertyOf <http://rdaregistry.info/Elements/e/P20233> ;
    skos:definition "Relates an expression to an expression that is a modification of a source expression."@en .

<http://rdaregistry.info/Elements/e/P20204>
    rdakit:instructionNumber "24.5" ;
    rdakit:toolkitDefinition "An expression used as the basis for a derivative expression."@en, "Expression servant de base à une expression dérivée."@fr, "Una expresión utilizada como base para una expresión derivada."@es ;
    rdakit:toolkitLabel "basada en (expresión)"@es, "based on (expression)"@en, "basé sur (expression)"@fr ;
    reg:hasSubproperty <http://rdaregistry.info/Elements/e/P20081>, <http://rdaregistry.info/Elements/e/P20121>, <http://rdaregistry.info/Elements/e/P20122>, <http://rdaregistry.info/Elements/e/P20135>, <http://rdaregistry.info/Elements/e/P20139>, <http://rdaregistry.info/Elements/e/P20140>, <http://rdaregistry.info/Elements/e/P20141>, <http://rdaregistry.info/Elements/e/P20152>, <http://rdaregistry.info/Elements/e/P20159>, <http://rdaregistry.info/Elements/e/P20179>, <http://rdaregistry.info/Elements/e/P20183>, <http://rdaregistry.info/Elements/e/P20184>, <http://rdaregistry.info/Elements/e/P20185>, <http://rdaregistry.info/Elements/e/P20186>, <http://rdaregistry.info/Elements/e/P20189>, <http://rdaregistry.info/Elements/e/P20190>, <http://rdaregistry.info/Elements/e/P20193>, <http://rdaregistry.info/Elements/e/P20194>, <http://rdaregistry.info/Elements/e/P20195>, <http://rdaregistry.info/Elements/e/object/P20204> ;
    reg:hasUnconstrained <http://rdaregistry.info/Elements/u/P60305> ;
    reg:lexicalAlias <http://rdaregistry.info/Elements/e/basedOnExpression.en> ;
    reg:name "basedOnExpression"@en ;
    reg:status <http://metadataregistry.org/uri/RegStatus/1001> ;
    a rdf:Property ;
    rdfs:domain <http://rdaregistry.info/Elements/c/C10006> ;
    rdfs:isDefinedBy <http://rdaregistry.info/Elements/e/> ;
    rdfs:label "is based on (expression)"@en ;
    rdfs:subPropertyOf <http://rdaregistry.info/Elements/e/P20233> ;
    skos:definition "Relates an expression to an expression used as the basis for a derivative expression."@en .

<http://rdaregistry.info/Elements/e/P20205>
    rdakit:toolkitLabel "relaterat uttryck"@sv ;
    reg:hasSubproperty <http://rdaregistry.info/Elements/e/P20232>, <http://rdaregistry.info/Elements/e/P20234>, <http://rdaregistry.info/Elements/e/datatype/P20205>, <http://rdaregistry.info/Elements/e/object/P20205> ;
    reg:hasUnconstrained <http://rdaregistry.info/Elements/u/P60313> ;
    reg:lexicalAlias <http://rdaregistry.info/Elements/e/relatedExpressionExpression.en> ;
    reg:name "relatedExpressionExpression"@en ;
    reg:status <http://metadataregistry.org/uri/RegStatus/1001> ;
    a rdf:Property ;
    rdfs:domain <http://rdaregistry.info/Elements/c/C10006> ;
    rdfs:isDefinedBy <http://rdaregistry.info/Elements/e/> ;
    rdfs:label "har relaterat uttryck"@sv, "has related expression (expression)"@en ;
    rdfs:subPropertyOf <http://rdaregistry.info/Elements/e/P20297> ;
    skos:definition "Relates an expression to an expression associated with an expression being described."@en .

<http://rdaregistry.info/Elements/e/P20206>
    rdakit:instructionNumber "7.16" ;
    rdakit:toolkitDefinition "An indication of content that updates or complements the primary content of an expression."@en, "Contenido (por j., un índice, una bibliografía, un apéndice) destinado a suplementar el contenido primario de un recurso."@es, "Contenu (par exemple, un index, une bibliographie, une annexe) conçu pour compléter le contenu principal d’une ressource."@fr ;
    rdakit:toolkitLabel "bihang"@sv, "contenido suplementario"@es, "contenu supplémentaire"@fr, "supplementary content"@en ;
    reg:hasUnconstrained <http://rdaregistry.info/Elements/u/P60485> ;
    reg:lexicalAlias <http://rdaregistry.info/Elements/e/supplementaryContent.en> ;
    reg:name "supplementaryContent"@en ;
    reg:status <http://metadataregistry.org/uri/RegStatus/1001> ;
    a rdf:Property ;
    rdfs:domain <http://rdaregistry.info/Elements/c/C10006> ;
    rdfs:isDefinedBy <http://rdaregistry.info/Elements/e/> ;
    rdfs:label "har bihang"@sv, "has supplementary content"@en ;
    skos:definition "Relates an expression to an indication of content that updates or complements the primary content of an expression."@en ;
    skos:scopeNote "Supplementary content may include an index, a bibliography, or an appendix."@en .

<http://rdaregistry.info/Elements/e/P20207>
    rdakit:instructionNumber "7.15" ;
    rdakit:toolkitDefinition "A presence of image content that accompanies the primary content of an expression."@en, "Contenido destinado a ilustrar el contenido primario de un recurso.."@es, "Contenu destiné à illustrer le contenu principal d’une ressource."@fr ;
    rdakit:toolkitLabel "contenido ilustrativo"@es, "contenu illustratif"@fr, "illustrative content"@en, "illustrativt innehåll"@sv ;
    reg:hasUnconstrained <http://rdaregistry.info/Elements/u/P60486> ;
    reg:lexicalAlias <http://rdaregistry.info/Elements/e/illustrativeContent.en> ;
    reg:name "illustrativeContent"@en ;
    reg:status <http://metadataregistry.org/uri/RegStatus/1001> ;
    a rdf:Property ;
    rdfs:domain <http://rdaregistry.info/Elements/c/C10006> ;
    rdfs:isDefinedBy <http://rdaregistry.info/Elements/e/> ;
    rdfs:label "har illustrativt innehåll"@sv, "has illustrative content"@en ;
    skos:definition "Relates an expression to a presence of one or more still images that accompany the primary content of an expression."@en ;
    skos:scopeNote "Tables containing only words and/or numerical data are excluded."@en .

<http://rdaregistry.info/Elements/e/P20208>
    rdakit:instructionNumber "7.14" ;
    rdakit:seeAlso <http://rdaregistry.info/Elements/e/P20007> ;
    rdakit:toolkitDefinition "An indication of content that provides alternative sensory modes to perceive the primary content of an expression."@en, "Contenido que ayuda a las personas con discapacidad sensorial para lograr una mayor comprensión de un contenido que su discapacidad les impide oir y ver en forma completa."@es, "Contenu permettant aux handicapés sensoriels une meilleure compréhension d’un contenu que leur handicap les empêche de voir ou d’entendre parfaitement."@fr ;
    rdakit:toolkitLabel "accessibility content"@en, "contenido con accesibilidad ampliada"@es, "contenu accessible"@fr, "komplement för tillgänglighet"@sv ;
    reg:hasUnconstrained <http://rdaregistry.info/Elements/u/P60487> ;
    reg:lexicalAlias <http://rdaregistry.info/Elements/e/accessibilityContent.en> ;
    reg:name "accessibilityContent"@en ;
    reg:status <http://metadataregistry.org/uri/RegStatus/1001> ;
    a rdf:Property ;
    rdfs:domain <http://rdaregistry.info/Elements/c/C10006> ;
    rdfs:isDefinedBy <http://rdaregistry.info/Elements/e/> ;
    rdfs:label "har komplement för tillgänglighet"@sv, "has accessibility content"@en ;
    skos:definition "Relates an expression to an indication of content that provides alternative sensory modes to perceive the primary content of an expression."@en ;
    skos:scopeNote "Accessibility content includes accessible labels, audio description, captioning, image description, sign language, and subtitles. Accessibility content does not include subtitles in a language different from the spoken content."@en .

<http://rdaregistry.info/Elements/e/P20209>
    rdakit:instructionNumber "7.20" ;
    rdakit:toolkitDefinition "A musical or physical layout of the content of an expression that is presented in the form of musical notation."@en, "La disposition musicale ou matérielle du contenu d’une ressource qui se présente sous la forme d’une notation musicale."@fr, "La presentación musical o física del contenido de un recurso que se presenta en forma de notación musical."@es ;
    rdakit:toolkitLabel "format för noterad musik"@sv, "format of notated music"@en, "formato de música notada"@es, "présentation de la musique notée"@fr ;
    reg:hasUnconstrained <http://rdaregistry.info/Elements/u/P60488> ;
    reg:lexicalAlias <http://rdaregistry.info/Elements/e/formatOfNotatedMusic.en> ;
    reg:name "formatOfNotatedMusic"@en ;
    reg:status <http://metadataregistry.org/uri/RegStatus/1001> ;
    a rdf:Property ;
    rdfs:domain <http://rdaregistry.info/Elements/c/C10006> ;
    rdfs:isDefinedBy <http://rdaregistry.info/Elements/e/> ;
    rdfs:label "har format för noterad musik"@sv, "has format of notated music"@en ;
    skos:definition "Relates an expression to a musical or physical layout of the content of an expression that is presented in the form of musical notation."@en .

<http://rdaregistry.info/Elements/e/P20210>
    rdakit:instructionNumber "7.27" ;
    rdakit:toolkitDefinition "An indication of mathematical data and other features of the cartographic content of an expression not recorded in statements of scale, projection, and coordinates."@en, "Datos matemáticos y otras características del contenido cartográfico de un recurso, que no se han registrado en las menciones de escala, proyección y coordenadas."@es, "Données mathématiques et autres particularités du contenu cartographique d’une ressource qui ne sont pas enregistrées dans les mentions d’échelle, de projection et de coordonnées."@fr ;
    rdakit:toolkitLabel "autres particularités du contenu cartographique"@fr, "other details of cartographic content"@en, "otros detalles del contenido cartográfico"@es, "övrig kartografisk data"@sv ;
    reg:hasUnconstrained <http://rdaregistry.info/Elements/u/P60498> ;
    reg:lexicalAlias <http://rdaregistry.info/Elements/e/otherDetailsOfCartographicContent.en> ;
    reg:name "otherDetailsOfCartographicContent"@en ;
    reg:status <http://metadataregistry.org/uri/RegStatus/1001> ;
    a rdf:Property ;
    rdfs:domain <http://rdaregistry.info/Elements/c/C10006> ;
    rdfs:isDefinedBy <http://rdaregistry.info/Elements/e/> ;
    rdfs:label "har övrig kartografisk data"@sv, "has other details of cartographic content"@en ;
    skos:definition "Relates an expression to an indication of mathematical data and other features of the cartographic content of an expression not recorded in statements of scale, projection, and coordinates."@en .

<http://rdaregistry.info/Elements/e/P20211>
    rdakit:instructionNumber "24.5" ;
    rdakit:toolkitDefinition "An expression of a work that has been updated, corrected, or expanded."@en, "Expression d’une œuvre qui a été mise à jour, corrigée ou augmentée."@fr, "Una expresión de una obra que fue actualizada, corregida o ampliada."@es ;
    rdakit:toolkitLabel "revisada como"@es, "revised as"@en, "révisé comme"@fr ;
    reg:hasSubproperty <http://rdaregistry.info/Elements/e/object/P20211> ;
    reg:hasUnconstrained <http://rdaregistry.info/Elements/u/P60245> ;
    reg:lexicalAlias <http://rdaregistry.info/Elements/e/revisedAs.en> ;
    reg:name "revisedAs"@en ;
    reg:status <http://metadataregistry.org/uri/RegStatus/1001> ;
    a rdf:Property ;
    rdfs:domain <http://rdaregistry.info/Elements/c/C10006> ;
    rdfs:isDefinedBy <http://rdaregistry.info/Elements/e/> ;
    rdfs:label "is revised as"@en ;
    rdfs:subPropertyOf <http://rdaregistry.info/Elements/e/P20203> ;
    skos:definition "Relates an expression to an expression of a work that has been updated, corrected, or expanded."@en .

<http://rdaregistry.info/Elements/e/P20212>
    rdakit:instructionNumber "24.5" ;
    rdakit:toolkitDefinition "An expression of a work formed from the coming together of two or more expressions."@en, "Expression d’une œuvre formée par l’assemblage de deux ou plusieurs expressions."@fr, "Una expresión de una obra formada de la unión de dos o más expresiones."@es ;
    rdakit:toolkitLabel "fusionada para formar (expresión)"@es, "fusionné pour former (expression)"@fr, "merged to form (expression)"@en ;
    reg:hasSubproperty <http://rdaregistry.info/Elements/e/object/P20212> ;
    reg:hasUnconstrained <http://rdaregistry.info/Elements/u/P60504> ;
    reg:lexicalAlias <http://rdaregistry.info/Elements/e/mergedToFormExpression.en> ;
    reg:name "mergedToFormExpression"@en ;
    reg:status <http://metadataregistry.org/uri/RegStatus/1001> ;
    a rdf:Property ;
    rdfs:domain <http://rdaregistry.info/Elements/c/C10006> ;
    rdfs:isDefinedBy <http://rdaregistry.info/Elements/e/> ;
    rdfs:label "is merged to form (expression)"@en ;
    rdfs:subPropertyOf <http://rdaregistry.info/Elements/e/P20169> ;
    skos:definition "Relates an expression to an expression of a work formed from the coming together of two or more expressions."@en .

<http://rdaregistry.info/Elements/e/P20213>
    rdakit:instructionNumber "7.25.5" ;
    rdakit:toolkitDefinition "An indication of supplemental information about scale."@en, "Información complementaria sobre la escala tal como una mención de medidas comparativas o la limitación de la escala a partes particulares del contenido de un recurso."@es, "Information complémentaire relative à l’échelle, comme un relevé de mesures comparatives ou une limitation de l’échelle à certaines portions du contenu."@fr ;
    rdakit:toolkitLabel "additional scale information"@en, "información adicional de la escala"@es, "information supplémentaire sur l’échelle"@fr, "övrig skalinformation"@sv ;
    reg:hasUnconstrained <http://rdaregistry.info/Elements/u/P60510> ;
    reg:lexicalAlias <http://rdaregistry.info/Elements/e/additionalScaleInformation.en> ;
    reg:name "additionalScaleInformation"@en ;
    reg:status <http://metadataregistry.org/uri/RegStatus/1001> ;
    a rdf:Property ;
    rdfs:domain <http://rdaregistry.info/Elements/c/C10006> ;
    rdfs:isDefinedBy <http://rdaregistry.info/Elements/e/> ;
    rdfs:label "har övrig skalinformation"@sv, "has additional scale information"@en ;
    rdfs:subPropertyOf <http://rdaregistry.info/Elements/e/P20228> ;
    skos:definition "Relates an expression to an indication of supplemental information about scale."@en ;
    skos:scopeNote "Additional scale information includes statement of comparative measurements or limitation of the scale to particular parts of the content of an expression."@en .

<http://rdaregistry.info/Elements/e/P20214>
    rdakit:instructionNumber "6.10" ;
    rdakit:toolkitDefinition "An earliest date associated with an expression."@en, "La date la plus ancienne associée à une expression."@fr, "La fecha más antigua asociada con una expresión."@es ;
    rdakit:toolkitLabel "date de l’expression"@fr, "date of expression"@en, "fecha de la expresión"@es ;
    reg:hasUnconstrained <http://rdaregistry.info/Elements/u/P60527> ;
    reg:lexicalAlias <http://rdaregistry.info/Elements/e/dateOfExpression.en> ;
    reg:name "dateOfExpression"@en ;
    reg:status <http://metadataregistry.org/uri/RegStatus/1001> ;
    a rdf:Property ;
    rdfs:domain <http://rdaregistry.info/Elements/c/C10006> ;
    rdfs:isDefinedBy <http://rdaregistry.info/Elements/e/> ;
    rdfs:label "has date of expression"@en ;
    skos:definition "Relates an expression to an earliest date associated with an expression."@en .

<http://rdaregistry.info/Elements/e/P20215>
    rdakit:instructionNumber "7.21" ;
    rdakit:toolkitDefinition "An instrument, voice, and/or ensemble used, or intended to be used, for performance of musical content."@en, "El instrumento, instrumentos, voz, voces, etc., utilizados para (o con el propósito de ser utilizados para) la ejecución del contenido musical."@es, "Le ou les instruments, la ou les voix, etc. utilisés (ou destinés à être utilisés) dans une exécution d’un contenu musical."@fr ;
    rdakit:toolkitLabel "distribution d’exécution d’un contenu musical"@fr, "medio de interpretación del contenido musical"@es, "medium of performance of musical content"@en ;
    reg:hasUnconstrained <http://rdaregistry.info/Elements/u/P60537> ;
    reg:lexicalAlias <http://rdaregistry.info/Elements/e/mediumOfPerformanceOfMusicalContent.en> ;
    reg:name "mediumOfPerformanceOfMusicalContent"@en ;
    reg:status <http://metadataregistry.org/uri/RegStatus/1001> ;
    a rdf:Property ;
    rdfs:domain <http://rdaregistry.info/Elements/c/C10006> ;
    rdfs:isDefinedBy <http://rdaregistry.info/Elements/e/> ;
    rdfs:label "has medium of performance of musical content"@en ;
    skos:definition "Relates an expression to an instrument, voice, or ensemble used, or intended to be used, for performance of musical content."@en .

<http://rdaregistry.info/Elements/e/P20216>
    rdakit:instructionNumber "7.26" ;
    rdakit:toolkitDefinition "A method or system used to represent the surface of the Earth or of a celestial sphere on a plane."@en, "El medio o sistema utilizado para representar la superficie de la Tierra o de una esfera celeste en un plano."@es, "La méthode ou le système utilisé pour représenter la surface de la Terre ou d’une sphère céleste sur un plan."@fr ;
    rdakit:toolkitLabel "kartprojektion"@sv, "projection d’un contenu cartographique"@fr, "projection of cartographic content"@en, "proyección del contenido cartográfico"@es ;
    reg:hasUnconstrained <http://rdaregistry.info/Elements/u/P60542> ;
    reg:lexicalAlias <http://rdaregistry.info/Elements/e/projectionOfCartographicContent.en> ;
    reg:name "projectionOfCartographicContent"@en ;
    reg:status <http://metadataregistry.org/uri/RegStatus/1001> ;
    a rdf:Property ;
    rdfs:domain <http://rdaregistry.info/Elements/c/C10006> ;
    rdfs:isDefinedBy <http://rdaregistry.info/Elements/e/> ;
    rdfs:label "har kartprojektion"@sv, "has projection of cartographic content"@en ;
    skos:definition "Relates an expression to a method or system used to represent the surface of the earth or of a celestial sphere on a plane."@en .

<http://rdaregistry.info/Elements/e/P20217>
    rdakit:instructionNumber "7.11" ;
    rdakit:toolkitDefinition "A place, date, or other information associated with the recording, filming, etc., of the content of an expression."@en, "El lugar y fecha asociados con la captura (i.e., grabación, filmación, etc.) del contenido de un recurso."@es, "Le lieu et la date associés à la captation (c’est-à-dire l’enregistrement, le tournage, etc.) du contenu de la ressource."@fr ;
    rdakit:toolkitLabel "capture information"@en, "inspelningsort och inspelningstid"@sv, "lieu et date de la captation"@fr, "lugar y fecha de captura"@es ;
    reg:hasUnconstrained <http://rdaregistry.info/Elements/u/P60555> ;
    reg:lexicalAlias <http://rdaregistry.info/Elements/e/captureInformation.en> ;
    reg:name "capture information"@en ;
    reg:status <http://metadataregistry.org/uri/RegStatus/1001> ;
    a rdf:Property ;
    rdfs:domain <http://rdaregistry.info/Elements/c/C10006> ;
    rdfs:isDefinedBy <http://rdaregistry.info/Elements/e/> ;
    rdfs:label "har inspelningsort och inspelningstid"@sv, "has capture information"@en ;
    skos:definition "Relates an expression to a place, date, or other information associated with the recording, filming, etc., of the content of an expression. "@en .

<http://rdaregistry.info/Elements/e/P20218>
    rdakit:instructionNumber "7.11.2" ;
    rdakit:toolkitDefinition "A place associated with the recording, filming, etc., of the content of an expression."@en, "El lugar asociado con la captura (i.e, grabación, filmación, etc.) del contenido del recurso."@es, "Le lieu associé à la captation (c’est-à-dire l’enregistrement, le tournage, etc.) du contenu d’une ressource."@fr ;
    rdakit:toolkitLabel "inspelningsort"@sv, "lieu de captation"@fr, "lugar de captura"@es, "place of capture"@en ;
    reg:hasUnconstrained <http://rdaregistry.info/Elements/u/P60556> ;
    reg:lexicalAlias <http://rdaregistry.info/Elements/e/placeOfCapture.en> ;
    reg:name "placeOfCapture"@en ;
    reg:status <http://metadataregistry.org/uri/RegStatus/1001> ;
    a rdf:Property ;
    rdfs:domain <http://rdaregistry.info/Elements/c/C10006> ;
    rdfs:isDefinedBy <http://rdaregistry.info/Elements/e/> ;
    rdfs:label "har inspelningsort"@sv, "has place of capture"@en ;
    skos:definition "Relates an expression to a place associated with the recording, filming, etc., of the content of an expression."@en .

<http://rdaregistry.info/Elements/e/P20219>
    rdakit:instructionNumber "7.22" ;
    rdakit:toolkitDefinition "A playing time, performance time, running time, etc., of the content of an expression."@en, "El tiempo de reproducción, el tiempo de interpretación, etc., del contenido de un recurso."@es, "La durée de lecture, de projection, etc. du contenu de la ressource."@fr ;
    rdakit:toolkitLabel "duración"@es, "duration"@en, "durée"@fr, "speltid"@sv ;
    reg:hasUnconstrained <http://rdaregistry.info/Elements/u/P60557> ;
    reg:lexicalAlias <http://rdaregistry.info/Elements/e/duration.en> ;
    reg:name "duration"@en ;
    reg:status <http://metadataregistry.org/uri/RegStatus/1001> ;
    a rdf:Property ;
    rdfs:domain <http://rdaregistry.info/Elements/c/C10006> ;
    rdfs:isDefinedBy <http://rdaregistry.info/Elements/e/> ;
    rdfs:label "har speltid"@sv, "has duration"@en ;
    skos:definition "Relates an expression to a playing time, performance time, running time, etc., of the content of an expression."@en .

<http://rdaregistry.info/Elements/e/P20220>
    reg:status <http://metadataregistry.org/uri/RegStatus/1008> ;
    a rdf:Property ;
    rdfs:isDefinedBy <http://rdaregistry.info/Elements/e/> ;
    rdfs:subPropertyOf <http://rdaregistry.info/Elements/e/P20224> .

<http://rdaregistry.info/Elements/e/P20221>
    reg:status <http://metadataregistry.org/uri/RegStatus/1008> ;
    a rdf:Property ;
    rdfs:isDefinedBy <http://rdaregistry.info/Elements/e/> ;
    rdfs:subPropertyOf <http://rdaregistry.info/Elements/e/P20224> .

<http://rdaregistry.info/Elements/e/P20222>
    reg:status <http://metadataregistry.org/uri/RegStatus/1008> ;
    a rdf:Property ;
    rdfs:isDefinedBy <http://rdaregistry.info/Elements/e/> ;
    rdfs:subPropertyOf <http://rdaregistry.info/Elements/e/P20224> .

<http://rdaregistry.info/Elements/e/P20223>
    reg:status <http://metadataregistry.org/uri/RegStatus/1008> ;
    a rdf:Property ;
    rdfs:isDefinedBy <http://rdaregistry.info/Elements/e/> ;
    rdfs:subPropertyOf <http://rdaregistry.info/Elements/e/P20224> .

<http://rdaregistry.info/Elements/e/P20224>
    rdakit:instructionNumber "7.17" ;
    rdakit:toolkitDefinition "A presence of colour, tone, etc., in the content of an expression."@en, "La presencia de color, tono, etc., en el contenido de un recurso."@es, "La présence de couleur, teinte, etc. dans le contenu d’une ressource."@fr ;
    rdakit:toolkitLabel "colour content"@en, "contenido a color"@es, "contenu de couleur"@fr, "färginnehåll"@sv ;
    reg:hasSubproperty <http://rdaregistry.info/Elements/e/P20220>, <http://rdaregistry.info/Elements/e/P20221>, <http://rdaregistry.info/Elements/e/P20222>, <http://rdaregistry.info/Elements/e/P20223> ;
    reg:hasUnconstrained <http://rdaregistry.info/Elements/u/P60558> ;
    reg:lexicalAlias <http://rdaregistry.info/Elements/e/colourContent.en> ;
    reg:name "colourContent"@en ;
    reg:status <http://metadataregistry.org/uri/RegStatus/1001> ;
    a rdf:Property ;
    rdfs:domain <http://rdaregistry.info/Elements/c/C10006> ;
    rdfs:isDefinedBy <http://rdaregistry.info/Elements/e/> ;
    rdfs:label "har färginnehåll"@sv, "has colour content"@en ;
    skos:definition "Relates an expression to a presence of colour, tone, etc., in the content of an expression."@en ;
    skos:scopeNote "Black, white, single colour shades of black, single colour tints of white, and single colour tones of gray are considered to be single colours."@en .

<http://rdaregistry.info/Elements/e/P20225>
    rdakit:instructionNumber "7.18" ;
    rdakit:toolkitDefinition "A presence or absence of sound in an expression."@en, "La presencia de sonido en un recurso, diferente al que consiste primariamente de sonido grabado."@es, "Le son présent dans une ressource qui n’est pas constituée principalement de son enregistré."@fr ;
    rdakit:toolkitLabel "contenido sonoro"@es, "contenu sonore"@fr, "ljudinnehåll"@sv, "sound content"@en ;
    reg:hasUnconstrained <http://rdaregistry.info/Elements/u/P60559> ;
    reg:lexicalAlias <http://rdaregistry.info/Elements/e/soundContent.en> ;
    reg:name "soundContent"@en ;
    reg:status <http://metadataregistry.org/uri/RegStatus/1001> ;
    a rdf:Property ;
    rdfs:domain <http://rdaregistry.info/Elements/c/C10006> ;
    rdfs:isDefinedBy <http://rdaregistry.info/Elements/e/> ;
    rdfs:label "har ljudinnehåll"@sv, "has sound content"@en ;
    skos:definition "Relates an expression to a presence or absence of sound in an expression."@en .

<http://rdaregistry.info/Elements/e/P20226>
    rdakit:instructionNumber "7.25.3" ;
    rdakit:toolkitDefinition "A ratio of horizontal distances in cartographic content of an expression to the actual distances they represent."@en, "La proporción de las distancias horizontales en el contenido cartográfico de un recurso con las distancias reales que representan."@es, "Le rapport entre les distances horizontales dans le contenu cartographique d’une ressource et les distances réelles qu’elles représentent."@fr ;
    rdakit:toolkitLabel "escala horizontal del contenido cartográfico"@es, "horizontal scale of cartographic content"@en, "échelle des longueurs d’un contenu cartographique"@fr ;
    reg:hasUnconstrained <http://rdaregistry.info/Elements/u/P60563> ;
    reg:lexicalAlias <http://rdaregistry.info/Elements/e/horizontalScaleOfCartographicContent.en> ;
    reg:name "horizontalScaleOfCartographicContent"@en ;
    reg:status <http://metadataregistry.org/uri/RegStatus/1001> ;
    a rdf:Property ;
    rdfs:domain <http://rdaregistry.info/Elements/c/C10006> ;
    rdfs:isDefinedBy <http://rdaregistry.info/Elements/e/> ;
    rdfs:label "has horizontal scale of cartographic content"@en ;
    rdfs:subPropertyOf <http://rdaregistry.info/Elements/e/P20228> ;
    skos:definition "Relates an expression to a ratio of horizontal distances in cartographic content of an expression to the actual distances they represent."@en .

<http://rdaregistry.info/Elements/e/P20227>
    rdakit:instructionNumber "7.25.2" ;
    rdakit:toolkitDefinition "A ratio of the dimensions of a still image or three-dimensional form contained or embodied in an expression to the dimensions of the thing that is represented."@en, "La proporción de las dimensiones de una imagen fija o forma tridimensional que está contenida o incorporada en un recurso con las dimensiones de la entidad que representa."@es, "Le rapport entre les dimensions d’une image fixe ou d’une forme tridimensionnelle, contenue ou matérialisée dans une ressource, et les dimensions de l’entité qu’elle représente."@fr ;
    rdakit:toolkitLabel "escala de una imagen fija o una forma tridimensional"@es, "scale of still image or three-dimensional form"@en, "skala för stillbild eller tredimensionell bild"@sv, "échelle d’une image fixe ou d’une forme tridimensionnelle"@fr ;
    reg:hasUnconstrained <http://rdaregistry.info/Elements/u/P60564> ;
    reg:lexicalAlias <http://rdaregistry.info/Elements/e/scaleOfStillImageOrThreeDimensionalForm.en> ;
    reg:name "scaleOfStillImageOrThreeDimensionalForm"@en ;
    reg:status <http://metadataregistry.org/uri/RegStatus/1001> ;
    a rdf:Property ;
    rdfs:domain <http://rdaregistry.info/Elements/c/C10006> ;
    rdfs:isDefinedBy <http://rdaregistry.info/Elements/e/> ;
    rdfs:label "har skala för stillbild eller tredimensionell bild"@sv, "has scale of still image or three-dimensional form"@en ;
    rdfs:subPropertyOf <http://rdaregistry.info/Elements/e/P20228> ;
    skos:definition "Relates an expression to a ratio of the dimensions of a still image or three-dimensional form contained or embodied in an expression to the dimensions of the thing that is represented."@en .

<http://rdaregistry.info/Elements/e/P20228>
    rdakit:instructionNumber "7.25" ;
    rdakit:toolkitDefinition "A ratio of the dimensions of the content of an image or three-dimensional form to the dimensions of the thing that is represented."@en, "La proporción de las dimensiones de una imagen o forma tridimensional incluida o incorporada en un recurso con las dimensiones de la entidad que representa."@es, "Le rapport entre les dimensions d’une image ou d’une forme tridimensionnelle, contenue ou matérialisée dans une ressource, et les dimensions de l’entité qu’elle représente."@fr ;
    rdakit:toolkitLabel "escala"@es, "scale"@en, "skala"@sv, "échelle"@fr ;
    reg:hasSubproperty <http://rdaregistry.info/Elements/e/P20213>, <http://rdaregistry.info/Elements/e/P20226>, <http://rdaregistry.info/Elements/e/P20227>, <http://rdaregistry.info/Elements/e/P20230> ;
    reg:hasUnconstrained <http://rdaregistry.info/Elements/u/P60565> ;
    reg:lexicalAlias <http://rdaregistry.info/Elements/e/scale.en> ;
    reg:name "scale"@en ;
    reg:status <http://metadataregistry.org/uri/RegStatus/1001> ;
    a rdf:Property ;
    rdfs:domain <http://rdaregistry.info/Elements/c/C10006> ;
    rdfs:isDefinedBy <http://rdaregistry.info/Elements/e/> ;
    rdfs:label "har skala"@sv, "has scale"@en ;
    skos:definition "Relates an expression to a ratio of the dimensions of the content of an image or three-dimensional form to the dimensions of the thing that is represented."@en ;
    skos:scopeNote "Scale can apply to horizontal, vertical, angular, and/or other measurements represented in an expression."@en .

<http://rdaregistry.info/Elements/e/P20229>
    rdakit:instructionNumber "7.19" ;
    rdakit:toolkitDefinition "A numerical ratio of the width to the height of a moving image."@en, "La relación de la anchura con la altura de una imagen móvil."@es, "Le rapport entre la largeur et la hauteur d’une image animée."@fr ;
    rdakit:toolkitLabel "aspect ratio"@en, "format de l’image"@fr, "proporción dimensional"@es ;
    reg:hasUnconstrained <http://rdaregistry.info/Elements/u/P60566> ;
    reg:lexicalAlias <http://rdaregistry.info/Elements/e/aspectRatioDesignation.en> ;
    reg:name "aspectRatio"@en ;
    reg:status <http://metadataregistry.org/uri/RegStatus/1001> ;
    a rdf:Property ;
    rdfs:domain <http://rdaregistry.info/Elements/c/C10006> ;
    rdfs:isDefinedBy <http://rdaregistry.info/Elements/e/> ;
    rdfs:label "has aspect ratio"@en ;
    skos:definition "Relates an expression to a numerical ratio of the width to the height of a moving image."@en .

<http://rdaregistry.info/Elements/e/P20230>
    rdakit:instructionNumber "7.25.4" ;
    rdakit:toolkitDefinition "A scale of elevation or vertical dimension of cartographic content of an expression."@en, "La escala de elevación o dimensión vertical del contenido cartográfico de un recurso."@es, "L’échelle de l’élévation ou de la dimension verticale du contenu cartographique d’une ressource."@fr ;
    rdakit:toolkitLabel "escala vertical del contenido cartográfico"@es, "vertical scale of cartographic content"@en, "vertikal skala för kartografiskt innehåll"@sv, "échelle des hauteurs d’un contenu cartographique"@fr ;
    reg:hasUnconstrained <http://rdaregistry.info/Elements/u/P60579> ;
    reg:lexicalAlias <http://rdaregistry.info/Elements/e/verticalScaleOfCartographicContent.en> ;
    reg:name "verticalScaleOfCartographicContent"@en ;
    reg:status <http://metadataregistry.org/uri/RegStatus/1001> ;
    a rdf:Property ;
    rdfs:domain <http://rdaregistry.info/Elements/c/C10006> ;
    rdfs:isDefinedBy <http://rdaregistry.info/Elements/e/> ;
    rdfs:label "har vertikal skala för kartografiskt innehåll"@sv, "has vertical scale of cartographic content"@en ;
    rdfs:subPropertyOf <http://rdaregistry.info/Elements/e/P20228> ;
    skos:definition "Relates an expression to a scale of elevation or vertical dimension of cartographic content of an expression."@en .

<http://rdaregistry.info/Elements/e/P20231>
    rdakit:instructionNumber "17.6" ;
    rdakit:toolkitDefinition "A work realized through an expression."@en, "La obra realizada mediante una expresión"@es, "L’œuvre réalisée à travers une expression."@fr ;
    rdakit:toolkitLabel "obra expresada"@es, "uttryckt verk"@sv, "work expressed"@en, "œuvre exprimée"@fr ;
    reg:hasSubproperty <http://rdaregistry.info/Elements/e/object/P20231> ;
    reg:lexicalAlias <http://rdaregistry.info/Elements/e/workExpressed.en> ;
    reg:name "workExpressed"@en ;
    reg:status <http://metadataregistry.org/uri/RegStatus/1001> ;
    a rdf:Property ;
    rdfs:domain <http://rdaregistry.info/Elements/c/C10006> ;
    rdfs:isDefinedBy <http://rdaregistry.info/Elements/e/> ;
    rdfs:label "har uttryckt verk"@sv, "has work expressed"@en ;
    skos:definition "Relates an expression to a work realized through an expression."@en .

<http://rdaregistry.info/Elements/e/P20232>
    rdakit:instructionNumber "24.5" ;
    rdakit:toolkitDefinition "An expression of a work that is an augmentation of, or is augmented by, or is complemented by another expression."@en, "Expression d’une œuvre qui constitue une augmentation de l’expression ou qui est augmentée ou complétée par elle."@fr, "Una expresión de una obra que es un aumento de, o se ve aumentada por, o se complementa con la expresión."@es ;
    rdakit:toolkitLabel "accompanying expression relationship"@en, "relaciones de expresión acompañante"@es, "relation d’expression d’accompagnement"@fr ;
    reg:hasSubproperty <http://rdaregistry.info/Elements/e/P20100>, <http://rdaregistry.info/Elements/e/P20105>, <http://rdaregistry.info/Elements/e/P20192>, <http://rdaregistry.info/Elements/e/object/P20232> ;
    reg:hasUnconstrained <http://rdaregistry.info/Elements/u/P60709> ;
    reg:lexicalAlias <http://rdaregistry.info/Elements/e/accompanyingExpressionRelationship.en> ;
    reg:name "accompanyingExpressionRelationship"@en ;
    reg:status <http://metadataregistry.org/uri/RegStatus/1001> ;
    a rdf:Property ;
    rdfs:domain <http://rdaregistry.info/Elements/c/C10006> ;
    rdfs:isDefinedBy <http://rdaregistry.info/Elements/e/> ;
    rdfs:label "has accompanying expression relationship with"@en ;
    rdfs:subPropertyOf <http://rdaregistry.info/Elements/e/P20205> ;
    skos:definition "Relates an expression to an expression of a work that is an augmentation of, or is augmented by, or is complemented by another expression."@en .

<http://rdaregistry.info/Elements/e/P20233>
    rdakit:toolkitDefinition "An expression of a work that is based on or is a derivative of another expression."@en, "Expression d’une œuvre qui est basée sur l’expression ou en constitue un dérivé."@fr, "Una expresión de una obra que se basa en, o es una derivada de la expresión."@es ;
    rdakit:toolkitLabel "derivative expression relationship"@en, "relaciones de expresión derivada"@es, "relation d’expression dérivée"@fr ;
    reg:hasSubproperty <http://rdaregistry.info/Elements/e/P20203>, <http://rdaregistry.info/Elements/e/object/P20233> ;
    reg:lexicalAlias <http://rdaregistry.info/Elements/e/derivativeExpressionRelationship.en> ;
    reg:name "derivativeExpressionRelationship"@en ;
    reg:status <http://metadataregistry.org/uri/RegStatus/1001> ;
    a rdf:Property ;
    rdfs:isDefinedBy <http://rdaregistry.info/Elements/e/> ;
    rdfs:label "has derivative expression relationship"@en ;
    skos:definition "Relates an expression to an expression of a work that is based on or is a derivative of another expression."@en .

<http://rdaregistry.info/Elements/e/P20234>
    reg:hasSubproperty <http://rdaregistry.info/Elements/e/P20072>, <http://rdaregistry.info/Elements/e/P20202> ;
    reg:status <http://metadataregistry.org/uri/RegStatus/1008> ;
    a rdf:Property ;
    rdfs:isDefinedBy <http://rdaregistry.info/Elements/e/> ;
    rdfs:subPropertyOf <http://rdaregistry.info/Elements/e/P20205> .

<http://rdaregistry.info/Elements/e/P20235>
    rdakit:toolkitDefinition "An expression of a work that is preceded by or succeeded by another expression."@en, "Expression d’une œuvre qui est précédée ou suivie par l’expression."@fr, "Una expresión de una obra que es precedida por o sucedida por la expresión."@es ;
    rdakit:toolkitLabel "relaciones de expresión secuencial"@es, "relation d’expression séquentielle"@fr, "sequential expression relationship"@en ;
    reg:hasSubproperty <http://rdaregistry.info/Elements/e/P20154>, <http://rdaregistry.info/Elements/e/P20169>, <http://rdaregistry.info/Elements/e/object/P20235> ;
    reg:lexicalAlias <http://rdaregistry.info/Elements/e/sequentialExpressionRelationship.en> ;
    reg:name "sequentialExpressionRelationship"@en ;
    reg:status <http://metadataregistry.org/uri/RegStatus/1001> ;
    a rdf:Property ;
    rdfs:isDefinedBy <http://rdaregistry.info/Elements/e/> ;
    rdfs:label "has sequential expression relationship"@en ;
    skos:definition "Relates an expression to an expression of a work that is preceded by or succeeded by another expression."@en .

<http://rdaregistry.info/Elements/e/P20236>
    rdakit:toolkitDefinition "An expression that is contained in or contains another expression."@en, "Expression d’une œuvre qui est contenue dans l’expression ou la contient."@fr, "Una expresión que es incluida en, o contiene la expresión."@es ;
    rdakit:toolkitLabel "relación de la expresión todo-parte"@es, "relation d’expression tout-partie"@fr, "whole-part expression relationship"@en ;
    reg:hasSubproperty <http://rdaregistry.info/Elements/e/P20074>, <http://rdaregistry.info/Elements/e/P20145>, <http://rdaregistry.info/Elements/e/object/P20236> ;
    reg:lexicalAlias <http://rdaregistry.info/Elements/e/wholePartExpressionRelationship.en> ;
    reg:name "wholePartExpressionRelationship"@en ;
    reg:status <http://metadataregistry.org/uri/RegStatus/1001> ;
    a rdf:Property ;
    rdfs:isDefinedBy <http://rdaregistry.info/Elements/e/> ;
    rdfs:label "has whole-part expression relationship"@en ;
    skos:definition "Relates an expression to an expression that is contained in or contains another expression."@en .

<http://rdaregistry.info/Elements/e/P20237>
    rdakit:instructionNumber "18.5" ;
    rdakit:toolkitDefinition "An agent contributing to an expression of a work by providing an afterword to an original work."@en, "Personne, famille ou collectivité contribuant à une expression d’une œuvre en fournissant un après-propos à l’œuvre originale."@fr, "Una persona, familia o entidad corporativa que contribuye a una expresión de una obra proporcionando un epílogo a la obra original."@es ;
    rdakit:toolkitLabel "auteur d’après-propos"@fr, "escritor de epílogo"@es, "writer of afterword"@en ;
    reg:hasSubproperty <http://rdaregistry.info/Elements/e/object/P20237> ;
    reg:hasUnconstrained <http://rdaregistry.info/Elements/u/P60715> ;
    reg:lexicalAlias <http://rdaregistry.info/Elements/e/writerOfAfterword.en> ;
    reg:name "writerOfAfterword"@en ;
    reg:status <http://metadataregistry.org/uri/RegStatus/1001> ;
    a rdf:Property ;
    rdfs:domain <http://rdaregistry.info/Elements/c/C10006> ;
    rdfs:isDefinedBy <http://rdaregistry.info/Elements/e/> ;
    rdfs:label "has writer of afterword"@en ;
    rdfs:subPropertyOf <http://rdaregistry.info/Elements/e/P20046> ;
    skos:definition "Relates an expression to an agent contributing to an expression of a work by providing an afterword to an original work."@en .

<http://rdaregistry.info/Elements/e/P20238>
    rdakit:instructionNumber "18.5" ;
    rdakit:toolkitDefinition "An agent contributing to an expression of a work by providing a postface to an original work."@en, "Personne, famille ou collectivité contribuant à une expression d’une œuvre en fournissant une postface à l’œuvre originale."@fr, "Una persona, familia o entidad corporativa que contribuye a una expresión de una obra proporcionando unas palabras finales o conclusiones al original de la obra."@es ;
    rdakit:toolkitLabel "escritor de conclusión"@es, "postfacier"@fr, "writer of postface"@en ;
    reg:hasSubproperty <http://rdaregistry.info/Elements/e/object/P20238> ;
    reg:hasUnconstrained <http://rdaregistry.info/Elements/u/P60716> ;
    reg:lexicalAlias <http://rdaregistry.info/Elements/e/writerOfPostface.en> ;
    reg:name "writerOfPostface"@en ;
    reg:status <http://metadataregistry.org/uri/RegStatus/1001> ;
    a rdf:Property ;
    rdfs:domain <http://rdaregistry.info/Elements/c/C10006> ;
    rdfs:isDefinedBy <http://rdaregistry.info/Elements/e/> ;
    rdfs:label "has writer of postface"@en ;
    rdfs:subPropertyOf <http://rdaregistry.info/Elements/e/P20046> ;
    skos:definition "Relates an expression to an agent contributing to an expression of a work by providing a postface to an original work."@en .

<http://rdaregistry.info/Elements/e/P20239>
    rdakit:instructionNumber "24.5" ;
    rdakit:toolkitDefinition "An expression of a work that has been adapted as a musical theatre work."@en, "Expression d’une œuvre qui a été adaptée en œuvre de théâtre musical."@fr, "Una expresión de una obra que ha sido adaptada como una obra de teatro musical."@es ;
    rdakit:toolkitLabel "adaptación para teatro musical de (expresión)"@es, "adaptation au théâtre musical de (expression)"@fr, "musical theatre adaptation of (expression)"@en ;
    reg:hasSubproperty <http://rdaregistry.info/Elements/e/object/P20239> ;
    reg:hasUnconstrained <http://rdaregistry.info/Elements/u/P60719> ;
    reg:lexicalAlias <http://rdaregistry.info/Elements/e/musicalTheatreAdaptationOfExpression.en> ;
    reg:name "musicalTheatreAdaptationOfExpression"@en ;
    reg:status <http://metadataregistry.org/uri/RegStatus/1001> ;
    a rdf:Property ;
    rdfs:domain <http://rdaregistry.info/Elements/c/C10006> ;
    rdfs:isDefinedBy <http://rdaregistry.info/Elements/e/> ;
    rdfs:label "is musical theatre adaptation of (expression)"@en ;
    rdfs:subPropertyOf <http://rdaregistry.info/Elements/e/P20152> ;
    skos:definition "Relates an expression to an expression of a work that has been adapted as a musical theatre work."@en .

<http://rdaregistry.info/Elements/e/P20240>
    rdakit:instructionNumber "24.5" ;
    rdakit:toolkitDefinition "An expression of a work that has been adapted as an opera."@en, "Expression d’une œuvre qui a été adaptée à l’opéra."@fr, "Una expresión de una obra que ha sido adaptada como una ópera."@es ;
    rdakit:toolkitLabel "adaptación para ópera de (expresión)"@es, "adaptation à l’opéra de (expression)"@fr, "opera adaptation of (expression)"@en ;
    reg:hasSubproperty <http://rdaregistry.info/Elements/e/object/P20240> ;
    reg:hasUnconstrained <http://rdaregistry.info/Elements/u/P60720> ;
    reg:lexicalAlias <http://rdaregistry.info/Elements/e/operaAdaptationOfExpression.en> ;
    reg:name "operaAdaptationOfExpression"@en ;
    reg:status <http://metadataregistry.org/uri/RegStatus/1001> ;
    a rdf:Property ;
    rdfs:domain <http://rdaregistry.info/Elements/c/C10006> ;
    rdfs:isDefinedBy <http://rdaregistry.info/Elements/e/> ;
    rdfs:label "is opera adaptation of (expression)"@en ;
    rdfs:subPropertyOf <http://rdaregistry.info/Elements/e/P20152> ;
    skos:definition "Relates an expression to an expression of a work that has been adapted as an opera."@en .

<http://rdaregistry.info/Elements/e/P20241>
    rdakit:instructionNumber "24.5" ;
    rdakit:toolkitDefinition "An expression of a musical theatre work based on a source expression."@en, "Expression d’une œuvre de théâtre musical basée sur l’expression source."@fr, "Una expresión de una obra de teatro musical basada en la expresión fuente."@es ;
    rdakit:toolkitLabel "adaptada como teatro musical (expresión)"@es, "adapted as musical theatre (expression)"@en, "adapté au théâtre musical (expression)"@fr ;
    reg:hasSubproperty <http://rdaregistry.info/Elements/e/object/P20241> ;
    reg:hasUnconstrained <http://rdaregistry.info/Elements/u/P60721> ;
    reg:lexicalAlias <http://rdaregistry.info/Elements/e/adaptedAsMusicalTheatreExpression.en> ;
    reg:name "adaptedAsMusicalTheatreExpression"@en ;
    reg:status <http://metadataregistry.org/uri/RegStatus/1001> ;
    a rdf:Property ;
    rdfs:domain <http://rdaregistry.info/Elements/c/C10006> ;
    rdfs:isDefinedBy <http://rdaregistry.info/Elements/e/> ;
    rdfs:label "is adapted as musical theatre (expression)"@en ;
    rdfs:subPropertyOf <http://rdaregistry.info/Elements/e/P20153> ;
    skos:definition "Relates an expression to an expression of a musical theatre work based on a source expression."@en .

<http://rdaregistry.info/Elements/e/P20242>
    rdakit:instructionNumber "24.5" ;
    rdakit:toolkitDefinition "An expression of an opera based on a source expression."@en, "Expression d’un opéra basée sur l’expression source."@fr, "Una expresión de una ópera basada en la expresión fuente."@es ;
    rdakit:toolkitLabel "adaptada como ópera (expresión)"@es, "adapted as opera (expression)"@en, "adapté en opéra"@fr ;
    reg:hasSubproperty <http://rdaregistry.info/Elements/e/object/P20242> ;
    reg:hasUnconstrained <http://rdaregistry.info/Elements/u/P60722> ;
    reg:lexicalAlias <http://rdaregistry.info/Elements/e/adaptedAsOperaExpression.en> ;
    reg:name "adaptedAsOperaExpression"@en ;
    reg:status <http://metadataregistry.org/uri/RegStatus/1001> ;
    a rdf:Property ;
    rdfs:domain <http://rdaregistry.info/Elements/c/C10006> ;
    rdfs:isDefinedBy <http://rdaregistry.info/Elements/e/> ;
    rdfs:label "is adapted as opera (expression)"@en ;
    rdfs:subPropertyOf <http://rdaregistry.info/Elements/e/P20153> ;
    skos:definition "Relates an expression to an expression of an opera based on a source expression."@en .

<http://rdaregistry.info/Elements/e/P20243>
    rdakit:instructionNumber "24.5" ;
    rdakit:toolkitDefinition "An expression of a musical work that is used in a motion picture, play, television program, etc."@en, "Expression d’une œuvre musicale utilisée dans un film, une pièce de théâtre, une émission de télévision, etc."@fr, "Una expresión de una obra musical que se usa en una película cinematográfica, obra de teatro, programa de televisión, etc."@es ;
    rdakit:toolkitLabel "music (expression)"@en, "musique (expression)"@fr, "música (expresión)"@es ;
    reg:hasSubproperty <http://rdaregistry.info/Elements/e/P20085>, <http://rdaregistry.info/Elements/e/object/P20243> ;
    reg:hasUnconstrained <http://rdaregistry.info/Elements/u/P60723> ;
    reg:lexicalAlias <http://rdaregistry.info/Elements/e/musicExpression.en> ;
    reg:name "musicExpression"@en ;
    reg:status <http://metadataregistry.org/uri/RegStatus/1001> ;
    a rdf:Property ;
    rdfs:domain <http://rdaregistry.info/Elements/c/C10006> ;
    rdfs:isDefinedBy <http://rdaregistry.info/Elements/e/> ;
    rdfs:label "is music (expression)"@en ;
    rdfs:subPropertyOf <http://rdaregistry.info/Elements/e/P20100> ;
    skos:definition "Relates an expression to an expression of a musical work that is used in a motion picture, play, television program, etc."@en .

<http://rdaregistry.info/Elements/e/P20244>
    rdakit:instructionNumber "24.5" ;
    rdakit:toolkitDefinition "An expression of a work such as a motion picture, play, television program, etc. that uses a musical work."@en, "Expression d’une œuvre telle qu’un film, une pièce de théâtre, une émission de télévision, etc. qui utilise l’œuvre musicale."@fr, "Una expresión de una obra tal como una película cinematográfica, obra de teatro, programa de televisión, etc., que usa una obra musical."@es ;
    rdakit:toolkitLabel "music for (expression)"@en, "musique pour (expression)"@fr, "música de (expresión)"@es ;
    reg:hasSubproperty <http://rdaregistry.info/Elements/e/P20103>, <http://rdaregistry.info/Elements/e/object/P20244> ;
    reg:hasUnconstrained <http://rdaregistry.info/Elements/u/P60724> ;
    reg:lexicalAlias <http://rdaregistry.info/Elements/e/musicForExpression.en> ;
    reg:name "musicForExpression"@en ;
    reg:status <http://metadataregistry.org/uri/RegStatus/1001> ;
    a rdf:Property ;
    rdfs:domain <http://rdaregistry.info/Elements/c/C10006> ;
    rdfs:isDefinedBy <http://rdaregistry.info/Elements/e/> ;
    rdfs:label "is music for (expression)"@en ;
    rdfs:subPropertyOf <http://rdaregistry.info/Elements/e/P20100> ;
    skos:definition "Relates an expression to an expression of a work such as a motion picture, play, television program, etc., that uses a musical work."@en .

<http://rdaregistry.info/Elements/e/P20245>
    rdakit:instructionNumber "24.5" ;
    rdakit:toolkitDefinition "An expression of a musical work that is used in a video."@en, "Expression d’une œuvre musicale utilisée dans une vidéo."@fr, "Una expresión de una obra musical que es usada en un video."@es ;
    rdakit:toolkitLabel "musique de vidéo (expression)"@fr, "música de video (expresión)"@es, "video music (expression)"@en ;
    reg:hasSubproperty <http://rdaregistry.info/Elements/e/object/P20245> ;
    reg:hasUnconstrained <http://rdaregistry.info/Elements/u/P60725> ;
    reg:lexicalAlias <http://rdaregistry.info/Elements/e/videoMusicExpression.en> ;
    reg:name "videoMusicExpression"@en ;
    reg:status <http://metadataregistry.org/uri/RegStatus/1001> ;
    a rdf:Property ;
    rdfs:domain <http://rdaregistry.info/Elements/c/C10006> ;
    rdfs:isDefinedBy <http://rdaregistry.info/Elements/e/> ;
    rdfs:label "is video music (expression)"@en ;
    rdfs:subPropertyOf <http://rdaregistry.info/Elements/e/P20243> ;
    skos:definition "Relates an expression to an expression of a musical work that is used in a video."@en .

<http://rdaregistry.info/Elements/e/P20246>
    rdakit:instructionNumber "24.5" ;
    rdakit:toolkitDefinition "An expression of a work that uses a musical work in a video."@en, "Expression d’une œuvre qui utilise l’œuvre musicale dans une vidéo."@fr, "Una expresión de una obra que usa la obra musical en un video"@es ;
    rdakit:toolkitLabel "music for video (expression)"@en, "musique pour la vidéo (expression)"@fr, "música para video (expresión)"@es ;
    reg:hasSubproperty <http://rdaregistry.info/Elements/e/object/P20246> ;
    reg:hasUnconstrained <http://rdaregistry.info/Elements/u/P60726> ;
    reg:lexicalAlias <http://rdaregistry.info/Elements/e/musicForVideoExpression.en> ;
    reg:name "musicForVideoExpression"@en ;
    reg:status <http://metadataregistry.org/uri/RegStatus/1001> ;
    a rdf:Property ;
    rdfs:domain <http://rdaregistry.info/Elements/c/C10006> ;
    rdfs:isDefinedBy <http://rdaregistry.info/Elements/e/> ;
    rdfs:label "is music for video (expression)"@en ;
    rdfs:subPropertyOf <http://rdaregistry.info/Elements/e/P20244> ;
    skos:definition "Relates an expression to an expression of a work that uses a musical work in a video."@en .

<http://rdaregistry.info/Elements/e/P20247>
    rdakit:instructionNumber "24.5" ;
    rdakit:toolkitDefinition "An expression of a musical work that is used in a television program."@en, "Expression d’une œuvre musicale utilisée dans une émission de télévision."@fr, "Una expresión de una obra musical que es usada en un programa de televisión."@es ;
    rdakit:toolkitLabel "musique d’émission de télévision (expression)"@fr, "música de programa de televisión (expresión)"@es, "television program music (expression)"@en ;
    reg:hasSubproperty <http://rdaregistry.info/Elements/e/object/P20247> ;
    reg:hasUnconstrained <http://rdaregistry.info/Elements/u/P60727> ;
    reg:lexicalAlias <http://rdaregistry.info/Elements/e/televisionProgramMusicExpression.en> ;
    reg:name "televisionProgramMusicExpression"@en ;
    reg:status <http://metadataregistry.org/uri/RegStatus/1001> ;
    a rdf:Property ;
    rdfs:domain <http://rdaregistry.info/Elements/c/C10006> ;
    rdfs:isDefinedBy <http://rdaregistry.info/Elements/e/> ;
    rdfs:label "is television program music (expression)"@en ;
    rdfs:subPropertyOf <http://rdaregistry.info/Elements/e/P20243> ;
    skos:definition "Relates an expression to an expression of a musical work that is used in a television program."@en .

<http://rdaregistry.info/Elements/e/P20248>
    rdakit:instructionNumber "24.5" ;
    rdakit:toolkitDefinition "An expression of a work that uses a musical work in a television program."@en, "Expression d’une œuvre qui utilise l’œuvre musicale dans une émission de télévision."@fr, "Una expresión de una obra que usa la obra musical en un programa de televisión."@es ;
    rdakit:toolkitLabel "music for television program (expression)"@en, "musique pour l’émission de télévision (expression)"@fr, "música para programa de televisión (expresión)"@es ;
    reg:hasSubproperty <http://rdaregistry.info/Elements/e/object/P20248> ;
    reg:hasUnconstrained <http://rdaregistry.info/Elements/u/P60728> ;
    reg:lexicalAlias <http://rdaregistry.info/Elements/e/musicForTelevisionProgramExpression.en> ;
    reg:name "musicForTelevisionProgramExpression"@en ;
    reg:status <http://metadataregistry.org/uri/RegStatus/1001> ;
    a rdf:Property ;
    rdfs:domain <http://rdaregistry.info/Elements/c/C10006> ;
    rdfs:isDefinedBy <http://rdaregistry.info/Elements/e/> ;
    rdfs:label "is music for television program (expression)"@en ;
    rdfs:subPropertyOf <http://rdaregistry.info/Elements/e/P20244> ;
    skos:definition "Relates an expression to an expression of a work that uses a musical work in a television program."@en .

<http://rdaregistry.info/Elements/e/P20249>
    rdakit:instructionNumber "24.5" ;
    rdakit:toolkitDefinition "An expression of a musical work that is used in a radio program."@en, "Expression d’une œuvre musicale utilisée dans une émission de radio."@fr, "Una expresión de una obra musical que es usada en un programa radiofónico."@es ;
    rdakit:toolkitLabel "musique d’émission de radio (expression)"@fr, "música de programa radiofónico (expresión)"@es, "radio program music (expression)"@en ;
    reg:hasSubproperty <http://rdaregistry.info/Elements/e/object/P20249> ;
    reg:hasUnconstrained <http://rdaregistry.info/Elements/u/P60729> ;
    reg:lexicalAlias <http://rdaregistry.info/Elements/e/radioProgramMusicExpression.en> ;
    reg:name "radioProgramMusicExpression"@en ;
    reg:status <http://metadataregistry.org/uri/RegStatus/1001> ;
    a rdf:Property ;
    rdfs:domain <http://rdaregistry.info/Elements/c/C10006> ;
    rdfs:isDefinedBy <http://rdaregistry.info/Elements/e/> ;
    rdfs:label "is radio program music (expression)"@en ;
    rdfs:subPropertyOf <http://rdaregistry.info/Elements/e/P20243> ;
    skos:definition "Relates an expression to an expression of a musical work that is used in a radio program."@en .

<http://rdaregistry.info/Elements/e/P20250>
    rdakit:instructionNumber "24.5" ;
    rdakit:toolkitDefinition "An expression of a work that uses a musical work in a radio program."@en, "Expression d’une œuvre qui utilise l’œuvre musicale dans une émission de radio."@fr, "Una expresión de una obra que usa la obra musical en un programa radiofónico."@es ;
    rdakit:toolkitLabel "music for radio program (expression)"@en, "musique pour l’émission de radio (expression)"@fr, "música para programa radiofónico (expresión)"@es ;
    reg:hasSubproperty <http://rdaregistry.info/Elements/e/object/P20250> ;
    reg:hasUnconstrained <http://rdaregistry.info/Elements/u/P60730> ;
    reg:lexicalAlias <http://rdaregistry.info/Elements/e/musicForRadioProgramExpression.en> ;
    reg:name "musicForRadioProgramExpression"@en ;
    reg:status <http://metadataregistry.org/uri/RegStatus/1001> ;
    a rdf:Property ;
    rdfs:domain <http://rdaregistry.info/Elements/c/C10006> ;
    rdfs:isDefinedBy <http://rdaregistry.info/Elements/e/> ;
    rdfs:label "is music for radio program (expression)"@en ;
    rdfs:subPropertyOf <http://rdaregistry.info/Elements/e/P20244> ;
    skos:definition "Relates an expression to an expression of a work that uses a musical work in a radio program."@en .

<http://rdaregistry.info/Elements/e/P20251>
    rdakit:instructionNumber "24.5" ;
    rdakit:toolkitDefinition "An expression of a musical work that is used in a motion picture."@en, "Expression d’une œuvre musicale utilisée dans un film."@fr, "Una expresión de una obra musical que es usada en una película cinematográfica."@es ;
    rdakit:toolkitLabel "motion picture music (expression)"@en, "musique de film (expression)"@fr, "música de película cinematográfica (expresión)"@es ;
    reg:hasSubproperty <http://rdaregistry.info/Elements/e/object/P20251> ;
    reg:hasUnconstrained <http://rdaregistry.info/Elements/u/P60731> ;
    reg:lexicalAlias <http://rdaregistry.info/Elements/e/motionPictureMusicExpression.en> ;
    reg:name "motionPictureMusicExpression"@en ;
    reg:status <http://metadataregistry.org/uri/RegStatus/1001> ;
    a rdf:Property ;
    rdfs:domain <http://rdaregistry.info/Elements/c/C10006> ;
    rdfs:isDefinedBy <http://rdaregistry.info/Elements/e/> ;
    rdfs:label "is motion picture music (expression)"@en ;
    rdfs:subPropertyOf <http://rdaregistry.info/Elements/e/P20243> ;
    skos:definition "Relates an expression to an expression of a musical work that is used in a motion picture."@en .

<http://rdaregistry.info/Elements/e/P20252>
    rdakit:instructionNumber "24.5" ;
    rdakit:toolkitDefinition "An expression of a work that uses a musical work in a motion picture."@en, "Expression d’une œuvre qui utilise l’œuvre musicale dans un film."@fr, "Una expresión de una obra que usa la obra musical en una película cinematográfica."@es ;
    rdakit:toolkitLabel "music for motion picture (expression)"@en, "musique pour le film (expression)"@fr, "música para película cinematográfica (expresión)"@es ;
    reg:hasSubproperty <http://rdaregistry.info/Elements/e/object/P20252> ;
    reg:hasUnconstrained <http://rdaregistry.info/Elements/u/P60732> ;
    reg:lexicalAlias <http://rdaregistry.info/Elements/e/musicForMotionPictureExpression.en> ;
    reg:name "musicForMotionPictureExpression"@en ;
    reg:status <http://metadataregistry.org/uri/RegStatus/1001> ;
    a rdf:Property ;
    rdfs:domain <http://rdaregistry.info/Elements/c/C10006> ;
    rdfs:isDefinedBy <http://rdaregistry.info/Elements/e/> ;
    rdfs:label "is music for motion picture (expression)"@en ;
    rdfs:subPropertyOf <http://rdaregistry.info/Elements/e/P20244> ;
    skos:definition "Relates an expression to an expression of a work that uses a musical work in a motion picture."@en .

<http://rdaregistry.info/Elements/e/P20253>
    rdakit:instructionNumber "24.5" ;
    rdakit:toolkitDefinition "An expression of a work that provides choreography for use in a related expression."@en, "Expression d’une œuvre qui fournit la chorégraphie destinée à être utilisée dans l’expression en relation."@fr, "Una expresión de una obra que proporciona la coreografía para uso en la expresión relacionada."@es ;
    rdakit:toolkitLabel "choreography (expression)"@en, "chorégraphie (expression)"@fr, "coreografía (expresión)"@es ;
    reg:hasSubproperty <http://rdaregistry.info/Elements/e/object/P20253> ;
    reg:hasUnconstrained <http://rdaregistry.info/Elements/u/P60740> ;
    reg:lexicalAlias <http://rdaregistry.info/Elements/e/choreographyExpression.en> ;
    reg:name "choreographyExpression"@en ;
    reg:status <http://metadataregistry.org/uri/RegStatus/1001> ;
    a rdf:Property ;
    rdfs:domain <http://rdaregistry.info/Elements/c/C10006> ;
    rdfs:isDefinedBy <http://rdaregistry.info/Elements/e/> ;
    rdfs:label "is choreography (expression)"@en ;
    rdfs:subPropertyOf <http://rdaregistry.info/Elements/e/P20100> ;
    skos:definition "Relates an expression to an expression of a work that provides choreography for use in a related expression."@en .

<http://rdaregistry.info/Elements/e/P20254>
    rdakit:instructionNumber "24.5" ;
    rdakit:toolkitDefinition "An expression of a work that uses choreography of a related expression."@en, "Expression d’une œuvre qui utilise la chorégraphie de l’expression en relation."@fr, "Una expresión de una obra que usa la coreografía de la expresión relacionada."@es ;
    rdakit:toolkitLabel "choreography for (expression)"@en, "chorégraphie pour (expression)"@fr, "coreografía para (expresión)"@es ;
    reg:hasSubproperty <http://rdaregistry.info/Elements/e/object/P20254> ;
    reg:hasUnconstrained <http://rdaregistry.info/Elements/u/P60741> ;
    reg:lexicalAlias <http://rdaregistry.info/Elements/e/choreographyForExpression.en> ;
    reg:name "choreographyForExpression"@en ;
    reg:status <http://metadataregistry.org/uri/RegStatus/1001> ;
    a rdf:Property ;
    rdfs:domain <http://rdaregistry.info/Elements/c/C10006> ;
    rdfs:isDefinedBy <http://rdaregistry.info/Elements/e/> ;
    rdfs:label "is choreography for (expression)"@en ;
    rdfs:subPropertyOf <http://rdaregistry.info/Elements/e/P20100> ;
    skos:definition "Relates an expression to an expression of a work that uses choreography of a related expression."@en .

<http://rdaregistry.info/Elements/e/P20255>
    rdakit:instructionNumber "24.5" ;
    rdakit:toolkitDefinition "A graphic novel based on a source expression."@en, "Roman graphique basé sur l’expression source."@fr, "Una novela gráfica basada en la expresión fuente."@es ;
    rdakit:toolkitLabel "adaptada como novela gráfica (expresión)"@es, "adapted as graphic novel (expression)"@en, "adapté en roman graphique (expression)"@fr ;
    reg:hasSubproperty <http://rdaregistry.info/Elements/e/object/P20255> ;
    reg:hasUnconstrained <http://rdaregistry.info/Elements/u/P60742> ;
    reg:lexicalAlias <http://rdaregistry.info/Elements/e/adaptedAsGraphicNovelExpression.en> ;
    reg:name "adaptedAsGraphicNovelExpression"@en ;
    reg:status <http://metadataregistry.org/uri/RegStatus/1001> ;
    a rdf:Property ;
    rdfs:domain <http://rdaregistry.info/Elements/c/C10006> ;
    rdfs:isDefinedBy <http://rdaregistry.info/Elements/e/> ;
    rdfs:label "is adapted as graphic novel (expression)"@en ;
    rdfs:subPropertyOf <http://rdaregistry.info/Elements/e/P20153> ;
    skos:definition "Relates an expression to a graphic novel based on a source expression."@en .

<http://rdaregistry.info/Elements/e/P20256>
    rdakit:instructionNumber "24.5" ;
    rdakit:toolkitDefinition "An expression of a work that has been adapted as a graphic novel."@en, "Expression d’une œuvre qui a été adaptée en roman graphique."@fr, "Una expresión de una obra que ha sido adaptada como una novela gráfica."@es ;
    rdakit:toolkitLabel "adaptation en roman graphique de (expression)"@fr, "graphic novelization of (expression)"@en, "novelización gráfica de (expresión)"@es ;
    reg:hasSubproperty <http://rdaregistry.info/Elements/e/object/P20256> ;
    reg:hasUnconstrained <http://rdaregistry.info/Elements/u/P60743> ;
    reg:lexicalAlias <http://rdaregistry.info/Elements/e/graphicNovelizationOfExpression.en> ;
    reg:name "graphicNovelizationOfExpression"@en ;
    reg:status <http://metadataregistry.org/uri/RegStatus/1001> ;
    a rdf:Property ;
    rdfs:domain <http://rdaregistry.info/Elements/c/C10006> ;
    rdfs:isDefinedBy <http://rdaregistry.info/Elements/e/> ;
    rdfs:label "is graphic novelization of (expression)"@en ;
    rdfs:subPropertyOf <http://rdaregistry.info/Elements/e/P20152> ;
    skos:definition "Relates an expression to an expression of a work that has been adapted as a graphic novel."@en .

<http://rdaregistry.info/Elements/e/P20257>
    rdakit:instructionNumber "18.5" ;
    rdakit:toolkitDefinition "An agent contributing to an expression of a moving image work by designing and creating post-production visual effects."@en, "Personne, famille ou collectivité contribuant à une expression d’une œuvre d’images animées en concevant et en créant des effets visuels en postproduction."@fr, "Una persona, familia o entidad corporativa que contribuye a una expresión de una obra de imagen en movimiento desarrollando y creando efectos visuales de post-producción."@es ;
    rdakit:toolkitLabel "fournisseur d’effets visuels"@fr, "productor de efectos visuales"@es, "visual effects provider"@en ;
    reg:hasSubproperty <http://rdaregistry.info/Elements/e/object/P20257> ;
    reg:hasUnconstrained <http://rdaregistry.info/Elements/u/P60748> ;
    reg:lexicalAlias <http://rdaregistry.info/Elements/e/visualEffectsProvider.en> ;
    reg:name "visualEffectsProvider"@en ;
    reg:status <http://metadataregistry.org/uri/RegStatus/1001> ;
    a rdf:Property ;
    rdfs:domain <http://rdaregistry.info/Elements/c/C10006> ;
    rdfs:isDefinedBy <http://rdaregistry.info/Elements/e/> ;
    rdfs:label "has visual effects provider"@en ;
    rdfs:subPropertyOf <http://rdaregistry.info/Elements/e/P20053> ;
    skos:definition "Relates an expression to an agent contributing to an expression of a moving image work by designing and creating post-production visual effects."@en .

<http://rdaregistry.info/Elements/e/P20258>
    rdakit:instructionNumber "18.5" ;
    rdakit:toolkitDefinition "An agent contributing to an expression of a moving image or audio work by designing and creating on-set special effects such as on-set mechanical effects and in-camera optical effects."@en, "Personne, famille ou collectivité contribuant à une expression d’une œuvre d’images animées ou d’une œuvre audio en concevant et en créant des effets spéciaux de plateau (effets mécaniques de plateau et effets d’optique dans la caméra)."@fr, "Una persona, familia o entidad corporativa que contribuye a una expresión de una imagen en movimiento u obra sonora mediante el diseño y creación de efectos especiales del set (efectos mecánicos en el set y efectos ópticos en cámara)."@es ;
    rdakit:toolkitLabel "fournisseur d’effets spéciaux"@fr, "productor de efectos especiales"@es, "special effects provider"@en ;
    reg:hasSubproperty <http://rdaregistry.info/Elements/e/object/P20258> ;
    reg:hasUnconstrained <http://rdaregistry.info/Elements/u/P60749> ;
    reg:lexicalAlias <http://rdaregistry.info/Elements/e/specialEffectsProvider.en> ;
    reg:name "specialEffectsProvider"@en ;
    reg:status <http://metadataregistry.org/uri/RegStatus/1001> ;
    a rdf:Property ;
    rdfs:domain <http://rdaregistry.info/Elements/c/C10006> ;
    rdfs:isDefinedBy <http://rdaregistry.info/Elements/e/> ;
    rdfs:label "has special effects provider"@en ;
    rdfs:subPropertyOf <http://rdaregistry.info/Elements/e/P20053> ;
    skos:definition "Relates an expression to an agent contributing to an expression of a moving image or audio work by designing and creating on-set special effects such as on-set mechanical effects and in-camera optical effects."@en .

<http://rdaregistry.info/Elements/e/P20259>
    rdakit:instructionNumber "18.5" ;
    rdakit:toolkitDefinition "An illustrator contributing to an expression of a comic book, graphic novel, etc., by drawing the text and graphic sound effects."@en, "Illustrateur contribuant à une expression d’une bande dessinée, d’un roman graphique, etc. en dessinant le texte et les effets sonores graphiques."@fr, "Un ilustrador que contribuye a una expresión de un libro cómico, novela gráfica, etc., mediante el dibujo del texto y efectos de sonido gráfico."@es ;
    rdakit:toolkitLabel "letterer"@en, "lettreur"@fr, "rotulista"@es ;
    reg:hasSubproperty <http://rdaregistry.info/Elements/e/object/P20259> ;
    reg:hasUnconstrained <http://rdaregistry.info/Elements/u/P60750> ;
    reg:lexicalAlias <http://rdaregistry.info/Elements/e/letterer.en> ;
    reg:name "letterer"@en ;
    reg:status <http://metadataregistry.org/uri/RegStatus/1001> ;
    a rdf:Property ;
    rdfs:domain <http://rdaregistry.info/Elements/c/C10006> ;
    rdfs:isDefinedBy <http://rdaregistry.info/Elements/e/> ;
    rdfs:label "has letterer"@en ;
    rdfs:subPropertyOf <http://rdaregistry.info/Elements/e/P20051> ;
    skos:definition "Relates an expression to an illustrator contributing to an expression of a comic book, graphic novel, etc., by drawing the text and graphic sound effects."@en .

<http://rdaregistry.info/Elements/e/P20260>
    rdakit:instructionNumber "7.19.1.4.1.4" ;
    rdakit:toolkitDefinition "Details of the ratio of the width to the height of a moving image."@en, "Detalles de la relación de la anchura con la altura de una imagen móvil."@es ;
    rdakit:toolkitLabel "details of aspect ratio designation"@en, "detalles de la proporción dimensional"@es ;
    reg:hasUnconstrained <http://rdaregistry.info/Elements/u/P60760> ;
    reg:lexicalAlias <http://rdaregistry.info/Elements/e/detailsOfAspectRatioDesignation.en> ;
    reg:name "detailsOfAspectRatioDesignation"@en ;
    reg:status <http://metadataregistry.org/uri/RegStatus/1001> ;
    a rdf:Property ;
    rdfs:domain <http://rdaregistry.info/Elements/c/C10006> ;
    rdfs:isDefinedBy <http://rdaregistry.info/Elements/e/> ;
    rdfs:label "has details of aspect ratio designation"@en ;
    skos:definition "Relates an expression to details of the ratio of the width to the height of a moving image."@en .

<http://rdaregistry.info/Elements/e/P20261>
    rdakit:instructionNumber "7.17.1.4" ;
    rdakit:toolkitDefinition "Details of the presence of colour, tone, etc., in the content of an expression, and the specific colours, tones, etc., including black and white, present."@en, "Detalles de la presencia de color, tono, etc., y los colores específicos, tonos, etc. (incluyendo blanco y negro) presentes en el contenido de un recurso."@es ;
    rdakit:toolkitLabel "details of colour content"@en, "detaljerad information om färginnehåll"@sv, "detalles del contenido a color"@es ;
    reg:hasUnconstrained <http://rdaregistry.info/Elements/u/P60761> ;
    reg:lexicalAlias <http://rdaregistry.info/Elements/e/detailsOfColourContent.en> ;
    reg:name "detailsOfColourContent"@en ;
    reg:status <http://metadataregistry.org/uri/RegStatus/1001> ;
    a rdf:Property ;
    rdfs:domain <http://rdaregistry.info/Elements/c/C10006> ;
    rdfs:isDefinedBy <http://rdaregistry.info/Elements/e/> ;
    rdfs:label "har detaljerad information om färginnehåll"@sv, "has details of colour content"@en ;
    skos:definition "Relates an expression to details of the presence of colour, tone, etc., in the content of an expression, and the specific colours, tones, etc., including black and white, present."@en .

<http://rdaregistry.info/Elements/e/P20262>
    rdakit:instructionNumber "7.13.3.4" ;
    rdakit:toolkitDefinition "Details of the set of characters or symbols used to express musical content of an expression."@en, "Detalles del conjunto de caracteres y/o símbolos utilizados para expresar el contenido musical de un recurso."@es ;
    rdakit:toolkitLabel "details of form of musical notation"@en, "detaljerad information om form av musiknotation"@sv, "detalles de la forma de la notación musical"@es ;
    reg:hasUnconstrained <http://rdaregistry.info/Elements/u/P60762> ;
    reg:lexicalAlias <http://rdaregistry.info/Elements/e/detailsOfFormOfMusicalNotation.en> ;
    reg:name "detailsOfFormOfMusicalNotation"@en ;
    reg:status <http://metadataregistry.org/uri/RegStatus/1001> ;
    a rdf:Property ;
    rdfs:domain <http://rdaregistry.info/Elements/c/C10006> ;
    rdfs:isDefinedBy <http://rdaregistry.info/Elements/e/> ;
    rdfs:label "har detaljerad information om form av musiknotation"@sv, "has details of form of musical notation"@en ;
    skos:definition "Relates an expression to details of a set of characters or symbols used to express musical content of an expression."@en, "Relates an expression to details of the set of characters or symbols used to express musical content of an expression."@en .

<http://rdaregistry.info/Elements/e/P20263>
    rdakit:instructionNumber "7.13.5.4" ;
    rdakit:toolkitDefinition "Details of the set of characters or symbols used to express movement content of an expression."@en, "Detalles del conjunto de caracteres y/o símbolos usados para expresar el contenido de movimientos de un recurso."@es ;
    rdakit:toolkitLabel "details of form of notated movement"@en, "detaljerad information om form av noterad rörelse"@sv, "detalles de la forma de notación de movimientos"@es ;
    reg:hasUnconstrained <http://rdaregistry.info/Elements/u/P60763> ;
    reg:lexicalAlias <http://rdaregistry.info/Elements/e/detailsOfFormOfNotatedMovement.en> ;
    reg:name "detailsOfFormOfNotatedMovement"@en ;
    reg:status <http://metadataregistry.org/uri/RegStatus/1001> ;
    a rdf:Property ;
    rdfs:domain <http://rdaregistry.info/Elements/c/C10006> ;
    rdfs:isDefinedBy <http://rdaregistry.info/Elements/e/> ;
    rdfs:label "har detaljerad information om form av noterad rörelse"@sv, "has details of form of notated movement"@en ;
    skos:definition "Relates an expression to details of a set of characters or symbols used to express movement content of an expression."@en, "Relates an expression to details of the set of characters or symbols used to express movement content of an expression."@en .

<http://rdaregistry.info/Elements/e/P20264>
    rdakit:instructionNumber "7.20.1.4" ;
    rdakit:toolkitDefinition "Details of the musical or physical layout of the content of an expression that is presented in the form of musical notation."@en, "Detalles de la presentación musical o física del contenido de un recurso que se presenta en forma de notación musical."@es ;
    rdakit:toolkitLabel "details of format of notated music"@en, "detaljerad information om format för noterad musik"@sv, "detalles del formato de la música notada"@es ;
    reg:hasUnconstrained <http://rdaregistry.info/Elements/u/P60764> ;
    reg:lexicalAlias <http://rdaregistry.info/Elements/e/detailsOfFormatOfNotatedMusic.en> ;
    reg:name "detailsOfFormatOfNotatedMusic"@en ;
    reg:status <http://metadataregistry.org/uri/RegStatus/1001> ;
    a rdf:Property ;
    rdfs:domain <http://rdaregistry.info/Elements/c/C10006> ;
    rdfs:isDefinedBy <http://rdaregistry.info/Elements/e/> ;
    rdfs:label "har detaljerad information om format för noterad musik"@sv, "has details of format of notated music"@en ;
    skos:definition "Relates an expression to details of the musical or physical layout of the content of an expression that is presented in the form of musical notation."@en .

<http://rdaregistry.info/Elements/e/P20265>
    rdakit:instructionNumber "7.13.4.4" ;
    rdakit:toolkitDefinition "Details of the set of characters or symbols used to express the content of an expression in a form that can be perceived through touch."@en, "Detalles del conjunto de caracteres y/o símbolos utilizados para expresar el contenido de un recurso en tal forma que se pueda percibir mediante el tacto."@es ;
    rdakit:toolkitLabel "details of form of tactile notation"@en, "detaljerad information om form av taktil notation"@sv, "detalles de la forma de la notación táctil"@es ;
    reg:hasUnconstrained <http://rdaregistry.info/Elements/u/P60765> ;
    reg:lexicalAlias <http://rdaregistry.info/Elements/e/detailsOfFormOfTactileNotation.en> ;
    reg:name "detailsOfFormOfTactileNotation"@en ;
    reg:status <http://metadataregistry.org/uri/RegStatus/1001> ;
    a rdf:Property ;
    rdfs:domain <http://rdaregistry.info/Elements/c/C10006> ;
    rdfs:isDefinedBy <http://rdaregistry.info/Elements/e/> ;
    rdfs:label "har detaljerad information om form av taktil notation"@sv, "has details of form of tactile notation"@en ;
    skos:definition "Relates an expression to details of a set of characters or symbols used to express the content of an expression in a form that can be perceived through touch."@en, "Relates an expression to details of the set of characters or symbols used to express the content of an expression in a form that can be perceived through touch."@en .

<http://rdaregistry.info/Elements/e/P20266>
    rdakit:instructionNumber "7.13.2.4" ;
    rdakit:toolkitDefinition "Details of the set of characters or symbols used to express written language content of an expression."@en, "Detalles del conjunto de caracteres y/o símbolos usados para expresar el contenido de lengua escrita de un recurso."@es ;
    rdakit:toolkitLabel "details of script"@en, "detaljerad information om skriftart"@sv, "detalles de la escritura"@es ;
    reg:hasUnconstrained <http://rdaregistry.info/Elements/u/P60766> ;
    reg:lexicalAlias <http://rdaregistry.info/Elements/e/detailsOfScript.en> ;
    reg:name "detailsOfScript"@en ;
    reg:status <http://metadataregistry.org/uri/RegStatus/1001> ;
    a rdf:Property ;
    rdfs:domain <http://rdaregistry.info/Elements/c/C10006> ;
    rdfs:isDefinedBy <http://rdaregistry.info/Elements/e/> ;
    rdfs:label "har detaljerad information om skriftart"@sv, "has details of script"@en ;
    skos:definition "Relates an expression to details of a set of characters or symbols used to express written language content of an expression."@en, "Relates an expression to details of the set of characters or symbols used to express written language content of an expression."@en .

<http://rdaregistry.info/Elements/e/P20267>
    rdakit:instructionNumber "7.15.1.4" ;
    rdakit:toolkitDefinition "Details of content intended to illustrate the primary content of an expression."@en, "Detalles del contenido destinado a ilustrar el contenido primario de un recurso."@es ;
    rdakit:toolkitLabel "details of illustrative content"@en, "detaljerad information om illustrativt innehåll"@sv, "detalles del contenido ilustrativo"@es ;
    reg:hasUnconstrained <http://rdaregistry.info/Elements/u/P60804> ;
    reg:lexicalAlias <http://rdaregistry.info/Elements/e/detailsOfIllustrativeContent.en> ;
    reg:name "detailsOfIllustrativeContent"@en ;
    reg:status <http://metadataregistry.org/uri/RegStatus/1001> ;
    a rdf:Property ;
    rdfs:domain <http://rdaregistry.info/Elements/c/C10006> ;
    rdfs:isDefinedBy <http://rdaregistry.info/Elements/e/> ;
    rdfs:label "har detaljerad information om illustrativt innehåll"@sv, "has details of illustrative content"@en ;
    skos:definition "Relates an expression to details of content intended to illustrate the primary content of an expression."@en .

<http://rdaregistry.info/Elements/e/P20268>
    rdakit:toolkitDefinition "A work that is about an expression."@en, "Una obra que trata sobre la expresión."@es ;
    rdakit:toolkitLabel "materia de (expresión)"@es, "subject of (expression)"@en ;
    reg:hasSubproperty <http://rdaregistry.info/Elements/e/P20269>, <http://rdaregistry.info/Elements/e/object/P20268> ;
    reg:hasUnconstrained <http://rdaregistry.info/Elements/u/P60806> ;
    reg:lexicalAlias <http://rdaregistry.info/Elements/e/subjectOfExpression.en> ;
    reg:name "subjectOfExpression"@en ;
    reg:status <http://metadataregistry.org/uri/RegStatus/1001> ;
    a rdf:Property ;
    rdfs:domain <http://rdaregistry.info/Elements/c/C10006> ;
    rdfs:isDefinedBy <http://rdaregistry.info/Elements/e/> ;
    rdfs:label "is subject of (expression)"@en ;
    rdfs:subPropertyOf <http://rdaregistry.info/Elements/w/P10283> ;
    skos:definition "Relates an expression to a work that is about an expression."@en .

<http://rdaregistry.info/Elements/e/P20269>
    rdakit:instructionNumber "23.5" ;
    rdakit:toolkitDefinition "A work that describes a described expression."@en, "Expression d’une œuvre qui décrit une expression."@fr, "Una obra que describe una expresión descrita."@es ;
    rdakit:toolkitLabel "described in (expression)"@en, "descrita en (expresión)"@es, "décrit dans (expression)"@fr ;
    reg:hasSubproperty <http://rdaregistry.info/Elements/e/P20270>, <http://rdaregistry.info/Elements/e/P20271>, <http://rdaregistry.info/Elements/e/P20272>, <http://rdaregistry.info/Elements/e/P20273>, <http://rdaregistry.info/Elements/e/P20274>, <http://rdaregistry.info/Elements/e/object/P20269> ;
    reg:hasUnconstrained <http://rdaregistry.info/Elements/u/P60215> ;
    reg:lexicalAlias <http://rdaregistry.info/Elements/e/describedInExpression.en> ;
    reg:name "describedInExpression"@en ;
    reg:status <http://metadataregistry.org/uri/RegStatus/1001> ;
    a rdf:Property ;
    rdfs:domain <http://rdaregistry.info/Elements/c/C10006> ;
    rdfs:isDefinedBy <http://rdaregistry.info/Elements/e/> ;
    rdfs:label "is described in (expression)"@en ;
    rdfs:subPropertyOf <http://rdaregistry.info/Elements/e/P20268> ;
    skos:definition "Relates an expression to a work that describes a described expression."@en .

<http://rdaregistry.info/Elements/e/P20270>
    rdakit:instructionNumber "23.5" ;
    rdakit:toolkitDefinition "A work that examines a source expression to identify its components and their relations."@en, "Expression d’une œuvre qui examine l’expression source pour identifier ses composantes et leurs relations."@fr, "Una obra que examina la expresión fuente para identificar sus componentes y sus relaciones."@es ;
    rdakit:toolkitLabel "analizada en (expresión)"@es, "analysed in (expression)"@en, "analysé dans (expression)"@fr ;
    reg:hasSubproperty <http://rdaregistry.info/Elements/e/object/P20270> ;
    reg:hasUnconstrained <http://rdaregistry.info/Elements/u/P60219> ;
    reg:lexicalAlias <http://rdaregistry.info/Elements/e/analysedInExpression.en> ;
    reg:name "analysedInExpression"@en ;
    reg:status <http://metadataregistry.org/uri/RegStatus/1001> ;
    a rdf:Property ;
    rdfs:domain <http://rdaregistry.info/Elements/c/C10006> ;
    rdfs:isDefinedBy <http://rdaregistry.info/Elements/e/> ;
    rdfs:label "is analysed in (expression)"@en ;
    rdfs:subPropertyOf <http://rdaregistry.info/Elements/e/P20269> ;
    skos:definition "Relates an expression to a work that examines a source expression to identify its components and their relations."@en .

<http://rdaregistry.info/Elements/e/P20271>
    rdakit:instructionNumber "23.5" ;
    rdakit:toolkitDefinition "A work that contains a set of explanatory or critical notes on a described expression."@en, "Expression d’une œuvre qui contient un ensemble de notes explicatives ou critiques sur l’expression décrite."@fr, "Una obra que contiene un conjunto de notas críticas o explicativas de la expresión descrita."@es ;
    rdakit:toolkitLabel "comentario en (expresión)"@es, "commentaire dans (expression)"@fr, "commentary in (expression)"@en ;
    reg:hasSubproperty <http://rdaregistry.info/Elements/e/object/P20271> ;
    reg:hasUnconstrained <http://rdaregistry.info/Elements/u/P60213> ;
    reg:lexicalAlias <http://rdaregistry.info/Elements/e/commentaryInExpression.en> ;
    reg:name "commentaryInExpression"@en ;
    reg:status <http://metadataregistry.org/uri/RegStatus/1001> ;
    a rdf:Property ;
    rdfs:domain <http://rdaregistry.info/Elements/c/C10006> ;
    rdfs:isDefinedBy <http://rdaregistry.info/Elements/e/> ;
    rdfs:label "is commentary in (expression)"@en ;
    rdfs:subPropertyOf <http://rdaregistry.info/Elements/e/P20269> ;
    skos:definition "Relates an expression to a work that contains a set of explanatory or critical notes on a described expression."@en .

<http://rdaregistry.info/Elements/e/P20272>
    rdakit:instructionNumber "23.5" ;
    rdakit:toolkitDefinition "A work that contains a critical evaluation of a described expression."@en, "Expression d’une œuvre qui contient une évaluation critique de l’expression décrite."@fr, "Una obra que contiene una evaluación crítica de la expresión descrita."@es ;
    rdakit:toolkitLabel "criticada en (expresión)"@es, "critiqued in (expression)"@en, "critiqué dans (expression)"@fr ;
    reg:hasSubproperty <http://rdaregistry.info/Elements/e/object/P20272> ;
    reg:hasUnconstrained <http://rdaregistry.info/Elements/u/P60212> ;
    reg:lexicalAlias <http://rdaregistry.info/Elements/e/critiquedInExpression.en> ;
    reg:name "critiquedInExpression"@en ;
    reg:status <http://metadataregistry.org/uri/RegStatus/1001> ;
    a rdf:Property ;
    rdfs:domain <http://rdaregistry.info/Elements/c/C10006> ;
    rdfs:isDefinedBy <http://rdaregistry.info/Elements/e/> ;
    rdfs:label "is critiqued in (expression)"@en ;
    rdfs:subPropertyOf <http://rdaregistry.info/Elements/e/P20269> ;
    skos:definition "Relates an expression to a work that contains a critical evaluation of a described expression."@en .

<http://rdaregistry.info/Elements/e/P20273>
    rdakit:instructionNumber "23.5" ;
    rdakit:toolkitDefinition "A work that examines or judges a described expression."@en, "Expression d’une œuvre qui examine ou juge l’expression décrite."@fr, "Una obra que examina o juzga la expresión descrita."@es ;
    rdakit:toolkitLabel "evaluada en (expresión)"@es, "evaluated in (expression)"@en, "évalué dans (expression)"@fr ;
    reg:hasSubproperty <http://rdaregistry.info/Elements/e/object/P20273> ;
    reg:hasUnconstrained <http://rdaregistry.info/Elements/u/P60218> ;
    reg:lexicalAlias <http://rdaregistry.info/Elements/e/evaluatedInExpression.en> ;
    reg:name "evaluatedInExpression"@en ;
    reg:status <http://metadataregistry.org/uri/RegStatus/1001> ;
    a rdf:Property ;
    rdfs:domain <http://rdaregistry.info/Elements/c/C10006> ;
    rdfs:isDefinedBy <http://rdaregistry.info/Elements/e/> ;
    rdfs:label "is evaluated in (expression)"@en ;
    rdfs:subPropertyOf <http://rdaregistry.info/Elements/e/P20269> ;
    skos:definition "Relates an expression to a work that examines or judges a described expression."@en .

<http://rdaregistry.info/Elements/e/P20274>
    rdakit:instructionNumber "23.5" ;
    rdakit:toolkitDefinition "A work that contains a brief evaluation of a described expression."@en, "Expression d’une œuvre qui contient une brève évaluation de l’expression décrite."@fr, "Una obra que contiene una evaluación breve de la expresión descrita."@es ;
    rdakit:toolkitLabel "recensé dans (expression)"@fr, "reseñada en (expresión)"@es, "reviewed in (expression)"@en ;
    reg:hasSubproperty <http://rdaregistry.info/Elements/e/object/P20274> ;
    reg:hasUnconstrained <http://rdaregistry.info/Elements/u/P60211> ;
    reg:lexicalAlias <http://rdaregistry.info/Elements/e/reviewedInExpression.en> ;
    reg:name "reviewedInExpression"@en ;
    reg:status <http://metadataregistry.org/uri/RegStatus/1001> ;
    a rdf:Property ;
    rdfs:domain <http://rdaregistry.info/Elements/c/C10006> ;
    rdfs:isDefinedBy <http://rdaregistry.info/Elements/e/> ;
    rdfs:label "is reviewed in (expression)"@en ;
    rdfs:subPropertyOf <http://rdaregistry.info/Elements/e/P20269> ;
    skos:definition "Relates an expression to a work that contains a brief evaluation of a described expression."@en .

<http://rdaregistry.info/Elements/e/P20275>
    rdakit:instructionNumber "18.5" ;
    rdakit:toolkitDefinition "An agent contributing to an expression of a work by providing a foreword to an original work."@en, "Una persona, familia o entidad corporativa que contribuye a una expresión de una obra proporcionando un prólogo a la obra original."@es ;
    rdakit:toolkitLabel "escritor de prólogo"@es, "writer of foreword"@en ;
    reg:hasSubproperty <http://rdaregistry.info/Elements/e/object/P20275> ;
    reg:hasUnconstrained <http://rdaregistry.info/Elements/u/P60809> ;
    reg:lexicalAlias <http://rdaregistry.info/Elements/e/writerOfForeword.en> ;
    reg:name "writerOfForeword"@en ;
    reg:status <http://metadataregistry.org/uri/RegStatus/1001> ;
    a rdf:Property ;
    rdfs:domain <http://rdaregistry.info/Elements/c/C10006> ;
    rdfs:isDefinedBy <http://rdaregistry.info/Elements/e/> ;
    rdfs:label "has writer of foreword"@en ;
    rdfs:subPropertyOf <http://rdaregistry.info/Elements/e/P20046> ;
    skos:definition "Relates an expression to an agent contributing to an expression of a work by providing a foreword to an original work."@en .

<http://rdaregistry.info/Elements/e/P20276>
    rdakit:instructionNumber "18.5" ;
    rdakit:toolkitDefinition "An agent contributing to an expression of a work by designing and creating audio/sound components."@en, "Una persona, familia o entidad corporativa que contribuye a una expresión de una obra mediante el diseño y la creación de componentes de sonido."@es ;
    rdakit:toolkitLabel "diseñador de sonido"@es, "sound designer"@en ;
    reg:hasSubproperty <http://rdaregistry.info/Elements/e/object/P20276> ;
    reg:hasUnconstrained <http://rdaregistry.info/Elements/u/P60811> ;
    reg:lexicalAlias <http://rdaregistry.info/Elements/e/soundDesigner.en> ;
    reg:name "soundDesigner"@en ;
    reg:status <http://metadataregistry.org/uri/RegStatus/1001> ;
    a rdf:Property ;
    rdfs:domain <http://rdaregistry.info/Elements/c/C10006> ;
    rdfs:isDefinedBy <http://rdaregistry.info/Elements/e/> ;
    rdfs:label "has sound designer"@en ;
    rdfs:subPropertyOf <http://rdaregistry.info/Elements/e/P20053> ;
    skos:definition "Relates an expression to an agent contributing to an expression of a work by designing and creating audio/sound components."@en .

<http://rdaregistry.info/Elements/e/P20277>
    rdakit:instructionNumber "18.5" ;
    rdakit:toolkitDefinition "An agent contributing to an expression of a work by designing and creating lighting components."@en, "Una persona, familia o entidad corporativa que contribuye a una expresión de una obra mediante el diseño y la creación de componentes de iluminación."@es ;
    rdakit:toolkitLabel "diseñador de iluminación"@es, "lighting designer"@en ;
    reg:hasSubproperty <http://rdaregistry.info/Elements/e/object/P20277> ;
    reg:hasUnconstrained <http://rdaregistry.info/Elements/u/P60813> ;
    reg:lexicalAlias <http://rdaregistry.info/Elements/e/lightingDesigner.en> ;
    reg:name "lightingDesigner"@en ;
    reg:status <http://metadataregistry.org/uri/RegStatus/1001> ;
    a rdf:Property ;
    rdfs:domain <http://rdaregistry.info/Elements/c/C10006> ;
    rdfs:isDefinedBy <http://rdaregistry.info/Elements/e/> ;
    rdfs:label "has lighting designer"@en ;
    rdfs:subPropertyOf <http://rdaregistry.info/Elements/e/P20053> ;
    skos:definition "Relates an expression to an agent contributing to an expression of a work by designing and creating lighting components."@en .

<http://rdaregistry.info/Elements/e/P20278>
    rdakit:instructionNumber "7.22.1.5" ;
    rdakit:toolkitDefinition "Details of a playing time, running time, performance time, etc., of the content of an expression."@en, "Tiempo de reproducción, duración, interpretación, etc., del contenido de un recurso."@es ;
    rdakit:toolkitLabel "details of duration"@en, "detaljerad information om speltid"@sv, "detalles de duración"@es ;
    reg:hasUnconstrained <http://rdaregistry.info/Elements/u/P60823> ;
    reg:lexicalAlias <http://rdaregistry.info/Elements/e/detailsOfDuration.en> ;
    reg:name "detailsOfDuration"@en ;
    reg:status <http://metadataregistry.org/uri/RegStatus/1001> ;
    a rdf:Property ;
    rdfs:domain <http://rdaregistry.info/Elements/c/C10006> ;
    rdfs:isDefinedBy <http://rdaregistry.info/Elements/e/> ;
    rdfs:label "har detaljerad information om speltid"@sv, "has details of duration"@en ;
    skos:definition "Relates an expression to details of a playing time, running time, performance time, etc., of the content of an expression."@en .

<http://rdaregistry.info/Elements/e/P20279>
    rdakit:instructionNumber "18.5" ;
    rdakit:seeAlso <http://rdaregistry.info/Elements/e/P20013> ;
    rdakit:toolkitDefinition "An agent contributing to an expression of a nonfiction moving image work by taking an active role as a participant."@en, "Una persona, familia o entidad corporativa que contribuye a una expresión de una obra de no ficción de imagen en movimiento mediante la adopción de un papel activo como participante."@es ;
    rdakit:toolkitLabel "on-screen participant"@en, "participante en pantalla"@es ;
    reg:hasSubproperty <http://rdaregistry.info/Elements/e/object/P20279> ;
    reg:hasUnconstrained <http://rdaregistry.info/Elements/u/P60824> ;
    reg:lexicalAlias <http://rdaregistry.info/Elements/e/onScreenParticipant.en> ;
    reg:name "onScreenParticipant"@en ;
    reg:status <http://metadataregistry.org/uri/RegStatus/1001> ;
    a rdf:Property ;
    rdfs:domain <http://rdaregistry.info/Elements/c/C10006> ;
    rdfs:isDefinedBy <http://rdaregistry.info/Elements/e/> ;
    rdfs:label "has on-screen participant"@en ;
    rdfs:subPropertyOf <http://rdaregistry.info/Elements/e/P20053> ;
    skos:definition "Relates an expression to an agent contributing to an expression of a nonfiction moving image work by taking an active role as a participant."@en ;
    skos:scopeNote "Appearance on screen to provide contextual or background information is excluded."@en .

<http://rdaregistry.info/Elements/e/P20280>
    rdakit:instructionNumber "18.5" ;
    rdakit:toolkitDefinition "An agent contributing to an expression of a work by researching, designing, implementing, or testing software."@en, "Una persona, familia o entidad corporativa que contribuye a una expresión de una obra mediante la investigación, diseño, implementación, y la realización de pruebas del software."@es ;
    rdakit:toolkitLabel "desarrollador de software"@es, "software developer"@en ;
    reg:hasSubproperty <http://rdaregistry.info/Elements/e/object/P20280> ;
    reg:hasUnconstrained <http://rdaregistry.info/Elements/u/P60828> ;
    reg:lexicalAlias <http://rdaregistry.info/Elements/e/softwareDeveloper.en> ;
    reg:name "softwareDeveloper"@en ;
    reg:status <http://metadataregistry.org/uri/RegStatus/1001> ;
    a rdf:Property ;
    rdfs:domain <http://rdaregistry.info/Elements/c/C10006> ;
    rdfs:isDefinedBy <http://rdaregistry.info/Elements/e/> ;
    rdfs:label "has software developer"@en ;
    rdfs:subPropertyOf <http://rdaregistry.info/Elements/e/P20053> ;
    skos:definition "Relates an expression to an agent contributing to an expression of a work by researching, designing, implementing, or testing software."@en .

<http://rdaregistry.info/Elements/e/P20281>
    rdakit:instructionNumber "24.5" ;
    rdakit:toolkitDefinition "An expression of a work that has been adapted as an oratorio."@en, "Una expresión de una obra que ha sido adaptada como un oratorio."@es ;
    rdakit:toolkitLabel "adaptación para oratorio de (expresión)"@es, "oratorio adaptation of (expression)"@en ;
    reg:hasSubproperty <http://rdaregistry.info/Elements/e/object/P20281> ;
    reg:hasUnconstrained <http://rdaregistry.info/Elements/u/P60830> ;
    reg:lexicalAlias <http://rdaregistry.info/Elements/e/oratorioAdaptationOfExpression.en> ;
    reg:name "oratorioAdaptationOfExpression"@en ;
    reg:status <http://metadataregistry.org/uri/RegStatus/1001> ;
    a rdf:Property ;
    rdfs:domain <http://rdaregistry.info/Elements/c/C10006> ;
    rdfs:isDefinedBy <http://rdaregistry.info/Elements/e/> ;
    rdfs:label "is oratorio adaptation of (expression)"@en ;
    rdfs:subPropertyOf <http://rdaregistry.info/Elements/e/P20152> ;
    skos:definition "Relates an expression to an expression of a work that has been adapted as an oratorio."@en .

<http://rdaregistry.info/Elements/e/P20282>
    rdakit:instructionNumber "24.5" ;
    rdakit:toolkitDefinition "An expression of an oratorio based on a source expression."@en, "Una expresión de un oratorio basada en la expresión fuente."@es ;
    rdakit:toolkitLabel "adaptada como oratorio (expresión)"@es, "adapted as oratorio (expression)"@en ;
    reg:hasSubproperty <http://rdaregistry.info/Elements/e/object/P20282> ;
    reg:hasUnconstrained <http://rdaregistry.info/Elements/u/P60831> ;
    reg:lexicalAlias <http://rdaregistry.info/Elements/e/adaptedAsOratorioExpression.en> ;
    reg:name "adaptedAsOratorioExpression"@en ;
    reg:status <http://metadataregistry.org/uri/RegStatus/1001> ;
    a rdf:Property ;
    rdfs:domain <http://rdaregistry.info/Elements/c/C10006> ;
    rdfs:isDefinedBy <http://rdaregistry.info/Elements/e/> ;
    rdfs:label "is adapted as oratorio (expression)"@en ;
    rdfs:subPropertyOf <http://rdaregistry.info/Elements/e/P20153> ;
    skos:definition "Relates an expression to an expression of an oratorio based on a source expression."@en .

<http://rdaregistry.info/Elements/e/P20283>
    rdakit:instructionNumber "18.5" ;
    rdakit:toolkitDefinition "An agent contributing to an expression of a work by applying colour to drawings, prints, photographs, maps, moving images, etc."@en, "Una persona, familia o entidad corporativa que contribuye a una expresión de una obra aplicando color a los dibujos, grabados, fotografías, mapas, imágenes en movimiento, etc."@es ;
    rdakit:toolkitLabel "colorista"@es, "colourist"@en ;
    reg:hasSubproperty <http://rdaregistry.info/Elements/e/object/P20283> ;
    reg:hasUnconstrained <http://rdaregistry.info/Elements/u/P60838> ;
    reg:lexicalAlias <http://rdaregistry.info/Elements/e/colourist.en> ;
    reg:name "colourist"@en ;
    reg:status <http://metadataregistry.org/uri/RegStatus/1001> ;
    a rdf:Property ;
    rdfs:domain <http://rdaregistry.info/Elements/c/C10006> ;
    rdfs:isDefinedBy <http://rdaregistry.info/Elements/e/> ;
    rdfs:label "has colourist"@en ;
    rdfs:subPropertyOf <http://rdaregistry.info/Elements/e/P20053> ;
    skos:definition "Relates an expression to an agent contributing to an expression of a work by applying colour to drawings, prints, photographs, maps, moving images, etc."@en .

<http://rdaregistry.info/Elements/e/P20284>
    rdakit:instructionNumber "18.5" ;
    rdakit:toolkitDefinition "An agent contributing to an expression of a work by applying make-up and prosthetics for a moving image production or for a musical or dramatic presentation or entertainment."@en, "Una persona, familia o entidad corporativa que contribuye a una expresión de una obra mediante la aplicación de maquillaje y prótesis para una producción de imágenes en movimiento o para una presentación o espectáculo musical o dramático."@es ;
    rdakit:toolkitLabel "make-up artist"@en, "maquillador"@es ;
    reg:hasSubproperty <http://rdaregistry.info/Elements/e/object/P20284> ;
    reg:hasUnconstrained <http://rdaregistry.info/Elements/u/P60840> ;
    reg:lexicalAlias <http://rdaregistry.info/Elements/e/makeUpArtist.en> ;
    reg:name "makeUpArtist"@en ;
    reg:status <http://metadataregistry.org/uri/RegStatus/1001> ;
    a rdf:Property ;
    rdfs:domain <http://rdaregistry.info/Elements/c/C10006> ;
    rdfs:isDefinedBy <http://rdaregistry.info/Elements/e/> ;
    rdfs:label "has make-up artist"@en ;
    rdfs:subPropertyOf <http://rdaregistry.info/Elements/e/P20053> ;
    skos:definition "Relates an expression to an agent contributing to an expression of a work by applying make-up and prosthetics for a moving image production or for a musical or dramatic presentation or entertainment."@en .

<http://rdaregistry.info/Elements/e/P20285>
    rdakit:instructionNumber "18.5" ;
    rdakit:toolkitDefinition "A conductor contributing to an expression of a musical work by leading a choral performing group in a musical or dramatic presentation, etc."@en, "Un intérprete que contribuye a la expresión de una obra musical dirigiendo un grupo de interpretación coral en una presentación musical o teatral, etc."@es ;
    rdakit:toolkitLabel "choral conductor"@en, "director de coro"@es ;
    reg:hasSubproperty <http://rdaregistry.info/Elements/e/object/P20285> ;
    reg:hasUnconstrained <http://rdaregistry.info/Elements/u/P60842> ;
    reg:lexicalAlias <http://rdaregistry.info/Elements/e/choralConductor.en> ;
    reg:name "choralConductor"@en ;
    reg:status <http://metadataregistry.org/uri/RegStatus/1001> ;
    a rdf:Property ;
    rdfs:domain <http://rdaregistry.info/Elements/c/C10006> ;
    rdfs:isDefinedBy <http://rdaregistry.info/Elements/e/> ;
    rdfs:label "has choral conductor"@en ;
    rdfs:subPropertyOf <http://rdaregistry.info/Elements/e/P20011> ;
    skos:definition "Relates an expression to a conductor contributing to an expression of a musical work by leading a choral performing group in a musical or dramatic presentation, etc."@en .

<http://rdaregistry.info/Elements/e/P20286>
    rdakit:instructionNumber "18.5" ;
    rdakit:toolkitDefinition "A conductor contributing to an expression of a musical work by leading an instrumental performing group in a musical or dramatic presentation, etc."@en, "Un intérprete que contribuye a la expresión de una obra musical dirigiendo un grupo de interpretación instrumental en una presentación musical o teatral, etc."@es ;
    rdakit:toolkitLabel "director instrumental"@es, "instrumental conductor"@en ;
    reg:hasSubproperty <http://rdaregistry.info/Elements/e/object/P20286> ;
    reg:hasUnconstrained <http://rdaregistry.info/Elements/u/P60844> ;
    reg:lexicalAlias <http://rdaregistry.info/Elements/e/instrumentalConductor.en> ;
    reg:name "instrumentalConductor"@en ;
    reg:status <http://metadataregistry.org/uri/RegStatus/1001> ;
    a rdf:Property ;
    rdfs:domain <http://rdaregistry.info/Elements/c/C10006> ;
    rdfs:isDefinedBy <http://rdaregistry.info/Elements/e/> ;
    rdfs:label "has instrumental conductor"@en ;
    rdfs:subPropertyOf <http://rdaregistry.info/Elements/e/P20011> ;
    skos:definition "Relates an expression to a conductor contributing to an expression of a musical work by leading an instrumental performing group in a musical or dramatic presentation, etc."@en .

<http://rdaregistry.info/Elements/e/P20287>
    rdakit:instructionNumber "18.5" ;
    rdakit:seeAlso <http://rdaregistry.info/Elements/w/P10061> ;
    rdakit:toolkitDefinition "An agent contributing to an expression of a work by revising the content for the purpose of suppressing parts deemed objectionable on moral, political, military, or other grounds, but leaving the nature and content substantially unchanged."@en ;
    rdakit:toolkitLabel "censor"@en ;
    reg:hasSubproperty <http://rdaregistry.info/Elements/e/object/P20287> ;
    reg:hasUnconstrained <http://rdaregistry.info/Elements/u/P60851> ;
    reg:lexicalAlias <http://rdaregistry.info/Elements/e/censor.en> ;
    reg:name "censor"@en ;
    reg:status <http://metadataregistry.org/uri/RegStatus/1001> ;
    a rdf:Property ;
    rdfs:domain <http://rdaregistry.info/Elements/c/C10006> ;
    rdfs:isDefinedBy <http://rdaregistry.info/Elements/e/> ;
    rdfs:label "has censor"@en ;
    rdfs:subPropertyOf <http://rdaregistry.info/Elements/e/P20053> ;
    skos:definition "Relates an expression to an agent contributing to an expression of a work by revising the content for the purpose of suppressing parts deemed objectionable on moral, political, military, or other grounds, but leaving the nature and content substantially unchanged."@en ;
    skos:scopeNote "Substantial modification that results in the creation of a new work is excluded."@en .

<http://rdaregistry.info/Elements/e/P20288>
    rdakit:instructionNumber "18.5" ;
    rdakit:seeAlso <http://rdaregistry.info/Elements/w/P10056> ;
    rdakit:toolkitDefinition "An illustrator contributing to an expression of a work by providing supplementary photographic content to an original work."@en ;
    rdakit:toolkitLabel "photographer (expression)"@en ;
    reg:hasSubproperty <http://rdaregistry.info/Elements/e/object/P20288> ;
    reg:hasUnconstrained <http://rdaregistry.info/Elements/u/P60429> ;
    reg:lexicalAlias <http://rdaregistry.info/Elements/e/photographerExpression.en> ;
    reg:name "photographerExpression"@en ;
    reg:status <http://metadataregistry.org/uri/RegStatus/1001> ;
    a rdf:Property ;
    rdfs:domain <http://rdaregistry.info/Elements/c/C10006> ;
    rdfs:isDefinedBy <http://rdaregistry.info/Elements/e/> ;
    rdfs:label "has photographer (expression)"@en ;
    rdfs:subPropertyOf <http://rdaregistry.info/Elements/e/P20051> ;
    skos:definition "Relates an expression to an illustrator contributing to an expression of a work by providing supplementary photographic content to an original work."@en ;
    skos:scopeNote "Creation of content that is primarily artistic is excluded."@en .

<http://rdaregistry.info/Elements/e/P20289>
    rdakit:instructionNumber "18.5" ;
    rdakit:toolkitDefinition "An agent who contributes to an expression of a work by restoring and/or combining earlier expressions, which may be damaged or fragmentary, to create a new expression."@en ;
    rdakit:toolkitLabel "restorationist (expression)"@en ;
    reg:hasSubproperty <http://rdaregistry.info/Elements/e/object/P20289> ;
    reg:hasUnconstrained <http://rdaregistry.info/Elements/u/P60450> ;
    reg:lexicalAlias <http://rdaregistry.info/Elements/e/restorationistExpression.en> ;
    reg:name "restorationistExpression"@en ;
    reg:status <http://metadataregistry.org/uri/RegStatus/1001> ;
    a rdf:Property ;
    rdfs:domain <http://rdaregistry.info/Elements/c/C10006> ;
    rdfs:isDefinedBy <http://rdaregistry.info/Elements/e/> ;
    rdfs:label "has restorationist (expression)"@en ;
    rdfs:subPropertyOf <http://rdaregistry.info/Elements/e/P20053> ;
    skos:definition "Relates an expression to an agent who contributes to an expression of a work by restoring and/or combining earlier expressions, which may be damaged or fragmentary, to create a new expression."@en .

<http://rdaregistry.info/Elements/e/P20290>
    rdakit:instructionNumber "7.19.1.4" ;
    rdakit:toolkitDefinition "A general designation of the ratio of the width to the height of a moving image."@en ;
    rdakit:toolkitLabel "aspect ratio designation"@en ;
    reg:hasUnconstrained <http://rdaregistry.info/Elements/u/P60873> ;
    reg:lexicalAlias <http://rdaregistry.info/Elements/e/aspectRatioDesignation.en> ;
    reg:name "aspectRatioDesignation"@en ;
    reg:status <http://metadataregistry.org/uri/RegStatus/1001> ;
    a rdf:Property ;
    rdfs:domain <http://rdaregistry.info/Elements/c/C10006> ;
    rdfs:isDefinedBy <http://rdaregistry.info/Elements/e/> ;
    rdfs:label "has aspect ratio designation"@en ;
    skos:definition "Relates an expression to a general designation of the ratio of the width to the height of a moving image."@en .

<http://rdaregistry.info/Elements/e/P20291>
    rdakit:instructionNumber "7.25.6" ;
    rdakit:toolkitDefinition "A general designation of the lack of a ratio of the dimensions of the content of an image or three-dimensional form to the dimensions of the thing that is represented."@en ;
    rdakit:toolkitLabel "scale designation"@en ;
    reg:hasUnconstrained <http://rdaregistry.info/Elements/u/P60874> ;
    reg:lexicalAlias <http://rdaregistry.info/Elements/e/scaleDesignation.en> ;
    reg:name "scaleDesignation"@en ;
    reg:status <http://metadataregistry.org/uri/RegStatus/1001> ;
    a rdf:Property ;
    rdfs:domain <http://rdaregistry.info/Elements/c/C10006> ;
    rdfs:isDefinedBy <http://rdaregistry.info/Elements/e/> ;
    rdfs:label "has scale designation"@en ;
    skos:definition "Relates an expression to a general designation of the lack of a ratio of the dimensions of the content of an image or three-dimensional form to the dimensions of the thing that is represented."@en .

<http://rdaregistry.info/Elements/e/P20292>
    rdakit:instructionNumber "18.5" ;
    rdakit:toolkitDefinition "An agent contributing to the audio content of an expression by managing the technical aspects of sound during the processes of recording, mixing, and reproduction."@en ;
    rdakit:toolkitLabel "audio engineer"@en ;
    reg:hasSubproperty <http://rdaregistry.info/Elements/e/P20293>, <http://rdaregistry.info/Elements/e/object/P20292> ;
    reg:hasUnconstrained <http://rdaregistry.info/Elements/u/P60892> ;
    reg:lexicalAlias <http://rdaregistry.info/Elements/e/audioEngineer.en> ;
    reg:name "audioEngineer"@en ;
    reg:status <http://metadataregistry.org/uri/RegStatus/1001> ;
    a rdf:Property ;
    rdfs:domain <http://rdaregistry.info/Elements/c/C10006> ;
    rdfs:isDefinedBy <http://rdaregistry.info/Elements/e/> ;
    rdfs:label "has audio engineer"@en ;
    rdfs:subPropertyOf <http://rdaregistry.info/Elements/e/P20053> ;
    skos:definition "Relates an expression to an agent contributing to the audio content of an expression by managing the technical aspects of sound during the processes of recording, mixing, and reproduction."@en .

<http://rdaregistry.info/Elements/e/P20293>
    rdakit:instructionNumber "18.5" ;
    rdakit:seeAlso <http://rdaregistry.info/Elements/w/P10306> ;
    rdakit:toolkitDefinition "An audio engineer contributing to the audio content of an expression by manipulating, mixing, and assembling the multiple tracks of a recording."@en ;
    rdakit:toolkitLabel "mixing engineer"@en ;
    reg:hasSubproperty <http://rdaregistry.info/Elements/e/object/P20293> ;
    reg:hasUnconstrained <http://rdaregistry.info/Elements/u/P60893> ;
    reg:lexicalAlias <http://rdaregistry.info/Elements/e/mixingEngineer.en> ;
    reg:name "mixingEngineer"@en ;
    reg:status <http://metadataregistry.org/uri/RegStatus/1001> ;
    a rdf:Property ;
    rdfs:domain <http://rdaregistry.info/Elements/c/C10006> ;
    rdfs:isDefinedBy <http://rdaregistry.info/Elements/e/> ;
    rdfs:label "has mixing engineer"@en ;
    rdfs:subPropertyOf <http://rdaregistry.info/Elements/e/P20292> ;
    skos:definition "Relates an expression to an audio engineer contributing to the audio content of an expression by manipulating, mixing, and assembling the multiple tracks of a recording."@en ;
    skos:scopeNote "Remixing activities that substantially change the nature and content of the original work, resulting in a new work, are excluded."@en .

<http://rdaregistry.info/Elements/e/P20294>
    rdakit:instructionNumber "18.5" ;
    rdakit:seeAlso <http://rdaregistry.info/Elements/w/P10053> ;
    rdakit:toolkitDefinition "An agent contributing to an expression of a musical work by using electronic audio devices and/or computer software to generate sounds."@en ;
    rdakit:toolkitLabel "music programmer"@en ;
    reg:hasSubproperty <http://rdaregistry.info/Elements/e/object/P20294> ;
    reg:hasUnconstrained <http://rdaregistry.info/Elements/u/P60894> ;
    reg:lexicalAlias <http://rdaregistry.info/Elements/e/musicProgrammer.en> ;
    reg:name "musicProgrammer"@en ;
    reg:status <http://metadataregistry.org/uri/RegStatus/1001> ;
    a rdf:Property ;
    rdfs:domain <http://rdaregistry.info/Elements/c/C10006> ;
    rdfs:isDefinedBy <http://rdaregistry.info/Elements/e/> ;
    rdfs:label "has music programmer"@en ;
    rdfs:subPropertyOf <http://rdaregistry.info/Elements/e/P20053> ;
    skos:definition "Relates an expression to an agent contributing to an expression of a musical work by using electronic audio devices and/or computer software to generate sounds."@en, "Relates an expression to an agent contributing to an expression of a musical work by using electronic audio devices or computer software to generate sounds."@en ;
    skos:scopeNote "The creation of a new musical work is excluded."@en .

<http://rdaregistry.info/Elements/e/P20295>
    rdakit:instructionNumber "18.5" ;
    rdakit:toolkitDefinition "An agent responsible for the general management and supervision of the process of adding new dialogue or other sounds to complete a sound track for an expression."@en ;
    rdakit:toolkitLabel "dubbing director"@en ;
    reg:hasSubproperty <http://rdaregistry.info/Elements/e/object/P20295> ;
    reg:hasUnconstrained <http://rdaregistry.info/Elements/u/P60895> ;
    reg:lexicalAlias <http://rdaregistry.info/Elements/e/dubbingDirector.en> ;
    reg:name "dubbingDirector"@en ;
    reg:status <http://metadataregistry.org/uri/RegStatus/1001> ;
    a rdf:Property ;
    rdfs:domain <http://rdaregistry.info/Elements/c/C10006> ;
    rdfs:isDefinedBy <http://rdaregistry.info/Elements/e/> ;
    rdfs:label "has dubbing director"@en ;
    rdfs:subPropertyOf <http://rdaregistry.info/Elements/e/P20053> ;
    skos:definition "Relates an expression to an agent responsible for the general management and supervision of the process of adding new dialogue or other sounds to complete a sound track for an expression."@en .

<http://rdaregistry.info/Elements/e/P20296>
    rdakit:instructionNumber "18.5" ;
    rdakit:seeAlso <http://rdaregistry.info/Elements/e/P20293> ;
    rdakit:toolkitDefinition "An agent who mixes recorded tracks together during a live performance or in a recording studio to appear as one continuous track."@en ;
    rdakit:toolkitLabel "DJ"@en ;
    reg:hasSubproperty <http://rdaregistry.info/Elements/e/object/P20296> ;
    reg:hasUnconstrained <http://rdaregistry.info/Elements/u/P60896> ;
    reg:lexicalAlias <http://rdaregistry.info/Elements/e/DJ.en> ;
    reg:name "DJ"@en ;
    reg:status <http://metadataregistry.org/uri/RegStatus/1001> ;
    a rdf:Property ;
    rdfs:domain <http://rdaregistry.info/Elements/c/C10006> ;
    rdfs:isDefinedBy <http://rdaregistry.info/Elements/e/> ;
    rdfs:label "has DJ"@en ;
    rdfs:subPropertyOf <http://rdaregistry.info/Elements/e/P20053> ;
    skos:definition "Relates an expression to an agent who mixes recorded tracks together during a live performance or in a recording studio to appear as one continuous track."@en ;
    skos:scopeNote "Remixing activities that substantially change the nature and content of an original work, resulting in a new work, and mixing and assembling the multiple tracks of a recording are excluded."@en .

<http://rdaregistry.info/Elements/e/P20297>
    reg:hasSubproperty <http://rdaregistry.info/Elements/e/datatype/P20297>, <http://rdaregistry.info/Elements/e/object/P20297> ;
    reg:lexicalAlias <http://rdaregistry.info/Elements/e/relatedEntityExpression.en> ;
    reg:name "relatedEntityExpression"@en ;
    reg:status <http://metadataregistry.org/uri/RegStatus/1001> ;
    a rdf:Property ;
    rdfs:domain <http://rdaregistry.info/Elements/c/C10006> ;
    rdfs:isDefinedBy <http://rdaregistry.info/Elements/e/> ;
    rdfs:label "has related entity (expression)"@en ;
    rdfs:subPropertyOf <http://rdaregistry.info/Elements/x/P00001> ;
    skos:definition "Relates an expression to an entity associated with an expression being described."@en .

<http://rdaregistry.info/Elements/e/P20298>
    reg:hasSubproperty <http://rdaregistry.info/Elements/e/datatype/P20298>, <http://rdaregistry.info/Elements/e/object/P20298> ;
    reg:hasUnconstrained <http://rdaregistry.info/Elements/u/P60313> ;
    reg:lexicalAlias <http://rdaregistry.info/Elements/e/relatedWorkExpression.en> ;
    reg:name "relatedWorkExpression"@en ;
    reg:status <http://metadataregistry.org/uri/RegStatus/1001> ;
    a rdf:Property ;
    rdfs:domain <http://rdaregistry.info/Elements/c/C10006> ;
    rdfs:isDefinedBy <http://rdaregistry.info/Elements/e/> ;
    rdfs:label "has related work (expression)"@en ;
    rdfs:subPropertyOf <http://rdaregistry.info/Elements/e/P20297> ;
    skos:definition "Relates an expression to a work associated with an expression being described."@en .

<http://rdaregistry.info/Elements/e/P20299>
    reg:hasSubproperty <http://rdaregistry.info/Elements/e/datatype/P20299>, <http://rdaregistry.info/Elements/e/object/P20299> ;
    reg:hasUnconstrained <http://rdaregistry.info/Elements/u/P60313> ;
    reg:lexicalAlias <http://rdaregistry.info/Elements/e/relatedManifestationExpression.en> ;
    reg:name "relatedManifestationExpression"@en ;
    reg:status <http://metadataregistry.org/uri/RegStatus/1001> ;
    a rdf:Property ;
    rdfs:domain <http://rdaregistry.info/Elements/c/C10006> ;
    rdfs:isDefinedBy <http://rdaregistry.info/Elements/e/> ;
    rdfs:label "has related manifestation (expression)"@en ;
    rdfs:subPropertyOf <http://rdaregistry.info/Elements/e/P20297> ;
    skos:definition "Relates an expression to a manifestation associated with an expression being described."@en .

<http://rdaregistry.info/Elements/e/P20300>
    reg:hasSubproperty <http://rdaregistry.info/Elements/e/datatype/P20300>, <http://rdaregistry.info/Elements/e/object/P20300> ;
    reg:hasUnconstrained <http://rdaregistry.info/Elements/u/P60313> ;
    reg:lexicalAlias <http://rdaregistry.info/Elements/e/relatedItemExpression.en> ;
    reg:name "relatedItemExpression"@en ;
    reg:status <http://metadataregistry.org/uri/RegStatus/1001> ;
    a rdf:Property ;
    rdfs:domain <http://rdaregistry.info/Elements/c/C10006> ;
    rdfs:isDefinedBy <http://rdaregistry.info/Elements/e/> ;
    rdfs:label "has related item (expression)"@en ;
    rdfs:subPropertyOf <http://rdaregistry.info/Elements/e/P20297> ;
    skos:definition "Relates an expression to an item associated with an expression being described."@en .

<http://rdaregistry.info/Elements/e/P20301>
    reg:hasSubproperty <http://rdaregistry.info/Elements/e/datatype/P20301>, <http://rdaregistry.info/Elements/e/object/P20301> ;
    reg:lexicalAlias <http://rdaregistry.info/Elements/e/relatedAgentExpression.en> ;
    reg:name "relatedAgentExpression"@en ;
    reg:status <http://metadataregistry.org/uri/RegStatus/1001> ;
    a rdf:Property ;
    rdfs:domain <http://rdaregistry.info/Elements/c/C10006> ;
    rdfs:isDefinedBy <http://rdaregistry.info/Elements/e/> ;
    rdfs:label "has related agent (expression)"@en ;
    rdfs:subPropertyOf <http://rdaregistry.info/Elements/e/P20297> ;
    skos:definition "Relates an expression to an agent associated with an expression being described."@en .

<http://rdaregistry.info/Elements/e/P20302>
    reg:hasSubproperty <http://rdaregistry.info/Elements/e/datatype/P20302>, <http://rdaregistry.info/Elements/e/object/P20302> ;
    reg:lexicalAlias <http://rdaregistry.info/Elements/e/relatedPersonExpression.en> ;
    reg:name "relatedPersonExpression"@en ;
    reg:status <http://metadataregistry.org/uri/RegStatus/1001> ;
    a rdf:Property ;
    rdfs:domain <http://rdaregistry.info/Elements/c/C10006> ;
    rdfs:isDefinedBy <http://rdaregistry.info/Elements/e/> ;
    rdfs:label "has related person (expression)"@en ;
    rdfs:subPropertyOf <http://rdaregistry.info/Elements/e/P20301> ;
    skos:definition "Relates an expression to a person associated with an expression being described."@en .

<http://rdaregistry.info/Elements/e/P20303>
    reg:hasSubproperty <http://rdaregistry.info/Elements/e/datatype/P20303>, <http://rdaregistry.info/Elements/e/object/P20303> ;
    reg:lexicalAlias <http://rdaregistry.info/Elements/e/relatedFamilyExpression.en> ;
    reg:name "relatedFamilyExpression"@en ;
    reg:status <http://metadataregistry.org/uri/RegStatus/1001> ;
    a rdf:Property ;
    rdfs:domain <http://rdaregistry.info/Elements/c/C10006> ;
    rdfs:isDefinedBy <http://rdaregistry.info/Elements/e/> ;
    rdfs:label "has related family (expression)"@en ;
    rdfs:subPropertyOf <http://rdaregistry.info/Elements/e/P20305> ;
    skos:definition "Relates an expression to a family associated with an expression being described."@en .

<http://rdaregistry.info/Elements/e/P20304>
    reg:hasSubproperty <http://rdaregistry.info/Elements/e/datatype/P20304>, <http://rdaregistry.info/Elements/e/object/P20304> ;
    reg:lexicalAlias <http://rdaregistry.info/Elements/e/relatedCorporateBodyExpression.en> ;
    reg:name "relatedCorporateBodyExpression"@en ;
    reg:status <http://metadataregistry.org/uri/RegStatus/1001> ;
    a rdf:Property ;
    rdfs:domain <http://rdaregistry.info/Elements/c/C10006> ;
    rdfs:isDefinedBy <http://rdaregistry.info/Elements/e/> ;
    rdfs:label "has related corporate body (expression)"@en ;
    rdfs:subPropertyOf <http://rdaregistry.info/Elements/e/P20305> ;
    skos:definition "Relates an expression to a corporate body associated with an expression being described."@en .

<http://rdaregistry.info/Elements/e/P20305>
    reg:hasSubproperty <http://rdaregistry.info/Elements/e/datatype/P20305>, <http://rdaregistry.info/Elements/e/object/P20305> ;
    reg:lexicalAlias <http://rdaregistry.info/Elements/e/relatedCollectiveAgentExpression.en> ;
    reg:name "relatedCollectiveAgentExpression"@en ;
    reg:status <http://metadataregistry.org/uri/RegStatus/1001> ;
    a rdf:Property ;
    rdfs:domain <http://rdaregistry.info/Elements/c/C10006> ;
    rdfs:isDefinedBy <http://rdaregistry.info/Elements/e/> ;
    rdfs:label "has related collective agent (expression)"@en ;
    rdfs:subPropertyOf <http://rdaregistry.info/Elements/e/P20301> ;
    skos:definition "Relates an expression to a collective agent associated with an expression being described."@en .

<http://rdaregistry.info/Elements/e/P20306>
    reg:hasSubproperty <http://rdaregistry.info/Elements/e/datatype/P20306>, <http://rdaregistry.info/Elements/e/object/P20306> ;
    reg:lexicalAlias <http://rdaregistry.info/Elements/e/relatedPlaceExpression.en> ;
    reg:name "relatedPlaceExpression"@en ;
    reg:status <http://metadataregistry.org/uri/RegStatus/1001> ;
    a rdf:Property ;
    rdfs:domain <http://rdaregistry.info/Elements/c/C10006> ;
    rdfs:isDefinedBy <http://rdaregistry.info/Elements/e/> ;
    rdfs:label "has related place (expression)"@en ;
    rdfs:subPropertyOf <http://rdaregistry.info/Elements/e/P20297> ;
    skos:definition "Relates an expression to a place associated with an expression being described."@en .

<http://rdaregistry.info/Elements/e/P20307>
    reg:hasSubproperty <http://rdaregistry.info/Elements/e/datatype/P20307>, <http://rdaregistry.info/Elements/e/object/P20307> ;
    reg:lexicalAlias <http://rdaregistry.info/Elements/e/relatetdTimespanExpression.en> ;
    reg:name "relatetdTimespanExpression"@en ;
    reg:status <http://metadataregistry.org/uri/RegStatus/1001> ;
    a rdf:Property ;
    rdfs:domain <http://rdaregistry.info/Elements/c/C10006> ;
    rdfs:isDefinedBy <http://rdaregistry.info/Elements/e/> ;
    rdfs:label "has related time-span (expression)"@en ;
    rdfs:subPropertyOf <http://rdaregistry.info/Elements/e/P20297> ;
    skos:definition "Relates an expression to a time-span associated with an expression being described."@en .

<http://rdaregistry.info/Elements/e/P20308>
    reg:hasSubproperty <http://rdaregistry.info/Elements/e/datatype/P20308>, <http://rdaregistry.info/Elements/e/object/P20308> ;
    reg:lexicalAlias <http://rdaregistry.info/Elements/e/relatedNomenExpression.en> ;
    reg:name "relatedNomenExpression"@en ;
    reg:status <http://metadataregistry.org/uri/RegStatus/1001> ;
    a rdf:Property ;
    rdfs:domain <http://rdaregistry.info/Elements/c/C10006> ;
    rdfs:isDefinedBy <http://rdaregistry.info/Elements/e/> ;
    rdfs:label "has related nomen (expression)"@en ;
    rdfs:subPropertyOf <http://rdaregistry.info/Elements/e/P20297> ;
    skos:definition "Relates an expression to a nomen associated with an expression being described."@en .

<http://rdaregistry.info/Elements/e/P20309>
    rdakit:instructionNumber "7.11.4" ;
    rdakit:toolkitDefinition "A note providing information associated with the recording, filming, etc., of the content of an expression."@en ;
    rdakit:toolkitLabel "note on capture"@en ;
    reg:hasUnconstrained <http://rdaregistry.info/Elements/u/P60905> ;
    reg:lexicalAlias <http://rdaregistry.info/Elements/e/noteOnCapture.en> ;
    reg:name "noteOnCapture"@en ;
    reg:status <http://metadataregistry.org/uri/RegStatus/1001> ;
    a rdf:Property ;
    rdfs:domain <http://rdaregistry.info/Elements/c/C10006> ;
    rdfs:isDefinedBy <http://rdaregistry.info/Elements/e/> ;
    rdfs:label "has note on capture"@en ;
    rdfs:subPropertyOf <http://rdaregistry.info/Elements/e/P20071> ;
    skos:definition "Relates an expression to a note providing information associated with the recording, filming, etc., of the content of an expression."@en ;
    skos:scopeNote "Note on capture includes the circumstances such as a live or studio recording, the equipment used, etc."@en .

