@prefix rdf: <http://www.w3.org/1999/02/22-rdf-syntax-ns#> .
@prefix dc: <http://purl.org/dc/elements/1.1/> .
@prefix foaf: <http://xmlns.com/foaf/0.1/> .
@prefix rdakit: <http://metadataregistry.org/uri/profile/rdakit/> .
@prefix rdfs: <http://www.w3.org/2000/01/rdf-schema#> .
@prefix reg: <http://metadataregistry.org/uri/profile/regap/> .
@prefix skos: <http://www.w3.org/2004/02/skos/core#> .

<http://metadataregistry.org/uri/RegStatus/1001>
    a skos:Concept ;
    skos:prefLabel "Published"@en .

<http://metadataregistry.org/uri/RegStatus/1008>
    a skos:Concept ;
    skos:prefLabel "Deprecated"@en .

<http://rdaregistry.info/Elements/m/>
    dc:title "RDA Manifestation properties"@en ;
    skos:note "Properties derived from RDA elements and relationship designators with the domain of RDA Manifestation."@en ;
    foaf:homepage <http://www.rdaregistry.info/Elements/m/> .

<http://rdaregistry.info/Elements/m/P30001>
    rdakit:instructionNumber "3.3" ;
    rdakit:toolkitDefinition "A categorization reflecting the format of the storage medium and housing of a carrier in combination with the type of intermediation device required to view, play, run, etc., the content of a manifestation."@en, "Catégorisation reflétant le format du support de stockage et du contenant d’un support matériel combiné avec le type de dispositif de médiation requis pour visionner, faire fonctionner, faire défiler, etc. le contenu d’une ressource."@fr, "Una categorización que refleja el formato del medio de almacenamiento y alojamiento de un soporte en combinación con el tipo de aparato de intermediación requerido para ver, reproducir, operar, etc., el contenido de un recurso."@es ;
    rdakit:toolkitLabel "bärartyp"@sv, "carrier type"@en, "tipo de soporte"@es, "type de support matériel"@fr ;
    reg:hasUnconstrained <http://rdaregistry.info/Elements/u/P60048> ;
    reg:lexicalAlias <http://rdaregistry.info/Elements/m/carrierType.en> ;
    reg:name "carrierType"@en ;
    reg:status <http://metadataregistry.org/uri/RegStatus/1001> ;
    a rdf:Property ;
    rdfs:domain <http://rdaregistry.info/Elements/c/C10007> ;
    rdfs:isDefinedBy <http://rdaregistry.info/Elements/m/> ;
    rdfs:label "a pour type de support matériel"@fr, "har bärartyp"@sv, "has carrier type"@en ;
    skos:definition "Met une manifestation en relation avec une catégorisation reflétant le format du support de stockage et du contenant d’un support matériel combiné avec le type de dispositif de médiation requis pour visionner, faire fonctionner, faire défiler, etc. le contenu d’une ressource."@fr, "Relates a manifestation to a categorization reflecting the format of the storage medium and housing of a carrier in combination with the type of intermediation device required to view, play, run, etc., the content of a manifestation."@en .

<http://rdaregistry.info/Elements/m/P30002>
    rdakit:instructionNumber "3.2" ;
    rdakit:toolkitDefinition "A categorization reflecting the general type of intermediation device required to view, play, run, etc., the content of a manifestation."@en, "Catégorisation indiquant le type général de dispositif de médiation requis pour visionner, faire fonctionner, faire défiler, etc. le contenu d’une ressource."@fr, "Una categorización que refleja el tipo general de elemento de intermediación que se requiere para ver, reproducir, operar, etc., el contenido de un recurso."@es ;
    rdakit:toolkitLabel "media type"@en, "medietyp"@sv, "tipo de medio"@es, "type de média"@fr ;
    reg:hasUnconstrained <http://rdaregistry.info/Elements/u/P60050> ;
    reg:lexicalAlias <http://rdaregistry.info/Elements/m/mediaType.en> ;
    reg:name "mediaType"@en ;
    reg:status <http://metadataregistry.org/uri/RegStatus/1001> ;
    a rdf:Property ;
    rdfs:domain <http://rdaregistry.info/Elements/c/C10007> ;
    rdfs:isDefinedBy <http://rdaregistry.info/Elements/m/> ;
    rdfs:label "a pour type de média"@fr, "har medietyp"@sv, "has media type"@en ;
    skos:definition "Met une manifestation en relation avec une catégorisation indiquant le type général de dispositif de médiation requis pour visionner, faire fonctionner, faire défiler, etc. le contenu d’une ressource."@fr, "Relates a manifestation to a categorization reflecting the general type of intermediation device required to view, play, run, etc., the content of a manifestation."@en .

<http://rdaregistry.info/Elements/m/P30003>
    rdakit:instructionNumber "2.13" ;
    rdakit:toolkitDefinition "A categorization reflecting whether a manifestation is issued in one or more parts, the way it is updated, and whether its termination is predetermined or not."@en, "Catégorisation permettant de signaler si une ressource est publiée en une ou plusieurs parties, son mode de mise à jour et sa complétude visée."@fr, "Una categorización que refleja si un recurso está publicado en una o más partes, su forma de actualización y su terminación esperada."@es ;
    rdakit:toolkitLabel "mode de parution"@fr, "mode of issuance"@en, "modo de edición"@es, "utgivningssätt"@sv ;
    reg:hasUnconstrained <http://rdaregistry.info/Elements/u/P60051> ;
    reg:lexicalAlias <http://rdaregistry.info/Elements/m/modeOfIssuance.en> ;
    reg:name "modeOfIssuance"@en ;
    reg:status <http://metadataregistry.org/uri/RegStatus/1001> ;
    a rdf:Property ;
    rdfs:domain <http://rdaregistry.info/Elements/c/C10007> ;
    rdfs:isDefinedBy <http://rdaregistry.info/Elements/m/> ;
    rdfs:label "a pour mode de parution"@fr, "har utgivningssätt"@sv, "has mode of issuance"@en ;
    skos:definition "Met une manifestation en relation avec une catégorisation permettant de signaler si une ressource est publiée en une ou plusieurs parties, son mode de mise à jour et sa complétude visée."@fr, "Relates a manifestation to a categorization reflecting whether a manifestation is issued in one or more parts, the way it is updated, and whether its termination is predetermined or not."@en .

<http://rdaregistry.info/Elements/m/P30004>
    rdakit:instructionNumber "2.15" ;
    rdakit:toolkitDefinition "A character string associated with a manifestation that serves to differentiate a manifestation from other manifestations."@en, "Chaîne de caractères associée à une manifestation qui sert à distinguer cette manifestation d’autres manifestations."@fr, "Una cadena de caracteres asociada con una manifestación que sirve para diferenciar esa manifestación de otras manifestaciones."@es ;
    rdakit:toolkitLabel "identifiant de la manifestation"@fr, "identificador de la manifestación"@es, "identifier for manifestation"@en, "identifikator för manifestationen"@sv ;
    reg:hasSubproperty <http://rdaregistry.info/Elements/m/P30065>, <http://rdaregistry.info/Elements/m/P30066> ;
    reg:hasUnconstrained <http://rdaregistry.info/Elements/u/P60052> ;
    reg:lexicalAlias <http://rdaregistry.info/Elements/m/identifierForManifestation.en> ;
    reg:name "identifierForManifestation"@en ;
    reg:status <http://metadataregistry.org/uri/RegStatus/1001> ;
    a rdf:Property ;
    rdfs:domain <http://rdaregistry.info/Elements/c/C10007> ;
    rdfs:isDefinedBy <http://rdaregistry.info/Elements/m/> ;
    rdfs:label "a pour identifiant de la manifestation"@fr, "har identifikator för manifestationen"@sv, "has identifier for manifestation"@en ;
    skos:definition "Met une manifestation en relation avec une chaîne de caractères associée à une manifestation qui sert à distinguer cette manifestation d’autres manifestations."@fr, "Relates a manifestation to a character string associated with a manifestation that serves to differentiate a manifestation from other manifestations."@en ;
    skos:scopeNote "An identifier for the manifestation includes registered identifiers from internationally recognized schemes, other identifiers assigned by publishers and others following internally devised schemes, identifiers known as fingerprints constructed by combining groups of characters from specified pages of early printed resources, publisher's numbers for notated music, and plate numbers for notated music."@en .

<http://rdaregistry.info/Elements/m/P30005>
    rdakit:instructionNumber "2.16" ;
    rdakit:toolkitDefinition "A citation for a manifestation in the form preferred by a creator, publisher, custodian, indexing or abstracting service, etc."@en, "Citation d’une ressource sous la forme privilégiée par un créateur, un éditeur, un dépositaire, un service d’indexation ou d’analyse, etc."@fr, "Una cita de un recurso en la forma preferida por el creador, editor, custodio, servicio de indización y resúmenes, etc."@es ;
    rdakit:toolkitLabel "cita preferida"@es, "citation privilégiée"@fr, "föredragen referensform"@sv, "preferred citation"@en ;
    reg:hasUnconstrained <http://rdaregistry.info/Elements/u/P60057> ;
    reg:lexicalAlias <http://rdaregistry.info/Elements/m/preferredCitation.en> ;
    reg:name "preferredCitation"@en ;
    reg:status <http://metadataregistry.org/uri/RegStatus/1001> ;
    a rdf:Property ;
    rdfs:domain <http://rdaregistry.info/Elements/c/C10007> ;
    rdfs:isDefinedBy <http://rdaregistry.info/Elements/m/> ;
    rdfs:label "a pour citation privilégiée"@fr, "har föredragen referensform"@sv, "has preferred citation"@en ;
    skos:definition "Met une manifestation en relation avec une citation d’une ressource sous la forme privilégiée par un créateur, un éditeur, un dépositaire, un service d’indexation ou d’analyse, etc."@fr, "Relates a manifestation to a citation for a manifestation in the form preferred by a creator, publisher, custodian, indexing or abstracting service, etc."@en .

<http://rdaregistry.info/Elements/m/P30006>
    rdakit:instructionNumber "3.19.6" ;
    rdakit:toolkitDefinition "A designation for one or more regions of the world for which a videodisc or video game carrier has been encoded, indicating that playback is restricted to a device configured to decode it."@en, "Code identifiant la région du monde pour laquelle un vidéodisque a été encodé et empêchant le disque d’être lu sur un lecteur vendu dans une région différente."@fr, "Un código que identifica la región del mundo para la cual se codificó el videodisco DVD, para prevenir que el disco se use en un reproductor vendido en una región diferente."@es ;
    rdakit:toolkitLabel "code de région"@fr, "codificación regional"@es, "regional encoding"@en, "regionkod"@sv ;
    reg:hasUnconstrained <http://rdaregistry.info/Elements/u/P60059> ;
    reg:lexicalAlias <http://rdaregistry.info/Elements/m/regionalEncoding.en> ;
    reg:name "regionalEncoding"@en ;
    reg:status <http://metadataregistry.org/uri/RegStatus/1001> ;
    a rdf:Property ;
    rdfs:domain <http://rdaregistry.info/Elements/c/C10007> ;
    rdfs:isDefinedBy <http://rdaregistry.info/Elements/m/> ;
    rdfs:label "a pour code de région"@fr, "har regionkod"@sv, "has regional encoding"@en ;
    rdfs:subPropertyOf <http://rdaregistry.info/Elements/m/P30124> ;
    skos:definition "Met une manifestation en relation avec un code identifiant la région du monde pour laquelle un vidéodisque a été encodé et empêchant le disque d’être lu sur un lecteur vendu dans une région différente."@fr, "Relates a manifestation to a designation for one or more regions of the world for which a videodisc or video game carrier has been encoded, indicating that playback is restricted to a device configured to decode it."@en .

<http://rdaregistry.info/Elements/m/P30007>
    rdakit:instructionNumber "2.11" ;
    rdakit:toolkitDefinition "A date associated with a claim of protection under copyright or a similar regime."@en, "Date associée à une revendication de protection en vertu du copyright ou d’un régime similaire."@fr, "Una fecha asociada con el reclamo de protección bajo el régimen de derechos de autor o régimen similares."@es ;
    rdakit:toolkitLabel "copyright date"@en, "copyrightår"@sv, "date de copyright"@fr, "fecha de derechos de autor"@es ;
    reg:hasUnconstrained <http://rdaregistry.info/Elements/u/P60069> ;
    reg:lexicalAlias <http://rdaregistry.info/Elements/m/copyrightDate.en> ;
    reg:name "copyrightDate"@en ;
    reg:status <http://metadataregistry.org/uri/RegStatus/1001> ;
    a rdf:Property ;
    rdfs:domain <http://rdaregistry.info/Elements/c/C10007> ;
    rdfs:isDefinedBy <http://rdaregistry.info/Elements/m/> ;
    rdfs:label "a pour date de copyright"@fr, "har copyrightår"@sv, "has copyright date"@en ;
    skos:definition "Met une manifestation en relation avec une date associée à une revendication de protection en vertu du copyright ou d’un régime similaire."@fr, "Relates a manifestation to a date associated with a claim of protection under copyright or a similar regime."@en ;
    skos:scopeNote "Copyright dates include phonogram dates, that is, dates associated with claims of protection for audio recordings."@en, "Les dates de copyright comprennent les dates de phonogramme (c’est-à-dire les dates associées à des revendications de protection pour les enregistrements sonores, aussi appelées dates de protection)."@fr .

<http://rdaregistry.info/Elements/m/P30008>
    rdakit:instructionNumber "2.9.6" ;
    rdakit:toolkitDefinition "A date associated with the distribution of a manifestation in a published form."@en, "Date associée à la diffusion ou à la distribution d’une ressource sous une forme publiée."@fr, "Una fecha asociada con la distribución de un recurso publicado."@es ;
    rdakit:toolkitLabel "date de diffusion ou de distribution"@fr, "date of distribution"@en, "distributionstid"@sv, "fecha de distribución"@es ;
    reg:hasUnconstrained <http://rdaregistry.info/Elements/u/P60070> ;
    reg:lexicalAlias <http://rdaregistry.info/Elements/m/dateOfDistribution.en> ;
    reg:name "dateOfDistribution"@en ;
    reg:status <http://metadataregistry.org/uri/RegStatus/1001> ;
    a rdf:Property ;
    rdfs:domain <http://rdaregistry.info/Elements/c/C10007> ;
    rdfs:isDefinedBy <http://rdaregistry.info/Elements/m/> ;
    rdfs:label "a pour date de diffusion ou de distribution"@fr, "har distributionstid"@sv, "has date of distribution"@en ;
    skos:definition "Met une manifestation en relation avec une date associée à la diffusion ou à la distribution d’une ressource sous une forme publiée."@fr, "Relates a manifestation to a date associated with the distribution of a manifestation in a published form."@en .

<http://rdaregistry.info/Elements/m/P30009>
    rdakit:instructionNumber "2.7.6" ;
    rdakit:toolkitDefinition "A date associated with the inscription, fabrication, construction, etc., of a manifestation in an unpublished form."@en, "Date associée à la scription, la fabrication, la construction, etc. d’une ressource sous une forme non publiée."@fr, "Una fecha asociada con la inscripción, fabricación, construcción, etc., de un recurso producido en forma inédita."@es ;
    rdakit:toolkitLabel "date de production"@fr, "date of production"@en, "fecha de producción"@es, "produktionstid"@sv ;
    reg:hasUnconstrained <http://rdaregistry.info/Elements/u/P60071> ;
    reg:lexicalAlias <http://rdaregistry.info/Elements/m/dateOfProduction.en> ;
    reg:name "dateOfProduction"@en ;
    reg:status <http://metadataregistry.org/uri/RegStatus/1001> ;
    a rdf:Property ;
    rdfs:domain <http://rdaregistry.info/Elements/c/C10007> ;
    rdfs:isDefinedBy <http://rdaregistry.info/Elements/m/> ;
    rdfs:label "a pour date de production"@fr, "har produktionstid"@sv, "has date of production"@en ;
    skos:definition "Met une manifestation en relation avec une date associée à la scription, la fabrication, la construction, etc. d’une ressource sous une forme non publiée."@fr, "Relates a manifestation to a date associated with the inscription, fabrication, construction, etc., of a manifestation in an unpublished form."@en .

<http://rdaregistry.info/Elements/m/P30010>
    rdakit:instructionNumber "2.10.6" ;
    rdakit:toolkitDefinition "A date associated with the printing, duplicating, casting, etc., of a manifestation in a published form."@en, "Date associée à l’impression, à la reproduction, au moulage, etc. d’une ressource sous une forme publiée."@fr, "Una fecha asociada con la impresión, duplicación, armado, etc., de un recurso publicado."@es ;
    rdakit:toolkitLabel "date de fabrication"@fr, "date of manufacture"@en, "fecha de fabricación"@es, "tillverkningstid"@sv ;
    reg:hasUnconstrained <http://rdaregistry.info/Elements/u/P60072> ;
    reg:lexicalAlias <http://rdaregistry.info/Elements/m/dateOfManufacture.en> ;
    reg:name "dateOfManufacture"@en ;
    reg:status <http://metadataregistry.org/uri/RegStatus/1001> ;
    a rdf:Property ;
    rdfs:domain <http://rdaregistry.info/Elements/c/C10007> ;
    rdfs:isDefinedBy <http://rdaregistry.info/Elements/m/> ;
    rdfs:label "a pour date de fabrication"@fr, "har tillverkningstid"@sv, "has date of manufacture"@en ;
    skos:definition "Met une manifestation en relation avec une date associée à l’impression, à la reproduction, au moulage, etc. d’une ressource sous une forme publiée."@fr, "Relates a manifestation to a date associated with the printing, duplicating, casting, etc., of a manifestation in a published form."@en .

<http://rdaregistry.info/Elements/m/P30011>
    rdakit:instructionNumber "2.8.6" ;
    rdakit:toolkitDefinition "A date associated with the publication, release, or issuing of a manifestation."@en, "Date associée à la publication, la mise à disposition ou l’édition d’une ressource."@fr, "Una fecha asociada con la publicación, entrega o emisión de un recurso."@es ;
    rdakit:toolkitLabel "date de publication"@fr, "date of publication"@en, "fecha de publicación"@es, "utgivningstid"@sv ;
    reg:hasUnconstrained <http://rdaregistry.info/Elements/u/P60073> ;
    reg:lexicalAlias <http://rdaregistry.info/Elements/m/dateOfPublication.en> ;
    reg:name "dateOfPublication"@en ;
    reg:status <http://metadataregistry.org/uri/RegStatus/1001> ;
    a rdf:Property ;
    rdfs:domain <http://rdaregistry.info/Elements/c/C10007> ;
    rdfs:isDefinedBy <http://rdaregistry.info/Elements/m/> ;
    rdfs:label "a pour date de publication"@fr, "har utgivningstid"@sv, "has date of publication"@en ;
    skos:definition "Met une manifestation en relation avec une date associée à la publication, la mise à disposition ou l’édition d’une ressource."@fr, "Relates a manifestation to a date associated with the publication, release, or issuing of a manifestation."@en .

<http://rdaregistry.info/Elements/m/P30012>
    rdakit:instructionNumber "2.5.7" ;
    rdakit:toolkitDefinition "A designation of a named revision of an edition in a language or script that differs from that recorded in a designation of a named revision of an edition element."@en, "Indication d’une révision nommée d’une édition dans une langue et/ou une écriture différentes de celles enregistrées dans l’élément Indication d’une révision nommée d’une édition."@fr, "Una designación de una revisión dada de una edición en una lengua y/o escritura que difiere de la registrada en el elemento designación de una revisión mencionada de una edición"@es ;
    rdakit:toolkitLabel "designación paralela de una revisión mencionada de una edición"@es, "indication parallèle d’une révision nommée d’une édition"@fr, "parallel designation of named revision of edition"@en, "parallell påföljande upplageförteckning"@sv ;
    reg:hasUnconstrained <http://rdaregistry.info/Elements/u/P60077> ;
    reg:lexicalAlias <http://rdaregistry.info/Elements/m/parallelDesignationOfNamedRevisionOfEdition.en> ;
    reg:name "parallelDesignationOfNamedRevisionOfEdition"@en ;
    reg:status <http://metadataregistry.org/uri/RegStatus/1001> ;
    a rdf:Property ;
    rdfs:domain <http://rdaregistry.info/Elements/c/C10007> ;
    rdfs:isDefinedBy <http://rdaregistry.info/Elements/m/> ;
    rdfs:label "a pour indication parallèle d’une révision nommée d’une édition"@fr, "har parallell påföljande upplageförteckning"@sv, "has parallel designation of named revision of edition"@en ;
    skos:definition "Met une manifestation en relation avec une indication d’une révision nommée d’une édition dans une langue et/ou une écriture différentes de celles enregistrées dans l’élément Indication d’une révision nommée d’une édition."@fr, "Relates a manifestation to a designation of a named revision of an edition in a language or script that differs from that recorded in a designation of a named revision of an edition element."@en .

<http://rdaregistry.info/Elements/m/P30013>
    rdakit:instructionNumber "2.5.3" ;
    rdakit:toolkitDefinition "A designation of edition in a language or script that differs from that recorded in a designation of edition element."@en, "Indication d’édition dans une langue et/ou une écriture différentes de celles enregistrées dans l’élément Indication de l’édition"@fr, "Una designación de edición en una lengua y/o escritura que difiere de la registrada en el elemento designación de edición."@es ;
    rdakit:toolkitLabel "designación paralela de edición"@es, "indication parallèle de l’édition"@fr, "parallel designation of edition"@en, "parallell upplageförteckning"@sv ;
    reg:hasUnconstrained <http://rdaregistry.info/Elements/u/P60078> ;
    reg:lexicalAlias <http://rdaregistry.info/Elements/m/parallelDesignationOfEdition.en> ;
    reg:name "parallelDesignationOfEdition"@en ;
    reg:status <http://metadataregistry.org/uri/RegStatus/1001> ;
    a rdf:Property ;
    rdfs:domain <http://rdaregistry.info/Elements/c/C10007> ;
    rdfs:isDefinedBy <http://rdaregistry.info/Elements/m/> ;
    rdfs:label "a pour indication parallèle de l’édition"@fr, "har parallell upplageförteckning"@sv, "has parallel designation of edition"@en ;
    skos:definition "Met une manifestation en relation avec une indication d’édition dans une langue et/ou une écriture différentes de celles enregistrées dans l’élément Indication de l’édition"@fr, "Relates a manifestation to a designation of edition in a language or script that differs from that recorded in a designation of edition element."@en .

<http://rdaregistry.info/Elements/m/P30014>
    rdakit:instructionNumber "2.12.9" ;
    rdakit:toolkitDefinition "A designation of the sequencing of a part or parts within a series."@en, "Indication d’ordre séquentiel d’une ou de plusieurs parties à l’intérieur d’une collection."@fr, "Una designación de la secuencia de una parte o partes dentro de la serie."@es ;
    rdakit:toolkitLabel "numbering within series"@en, "numeración dentro de la serie"@es, "numrering inom serie"@sv, "numérotation au sein de la collection"@fr ;
    reg:hasUnconstrained <http://rdaregistry.info/Elements/u/P60081> ;
    reg:lexicalAlias <http://rdaregistry.info/Elements/m/numberingWithinSeries.en> ;
    reg:name "numberingWithinSeries"@en ;
    reg:status <http://metadataregistry.org/uri/RegStatus/1001> ;
    a rdf:Property ;
    rdfs:domain <http://rdaregistry.info/Elements/c/C10007> ;
    rdfs:isDefinedBy <http://rdaregistry.info/Elements/m/> ;
    rdfs:label "a pour numérotation au sein de la collection"@fr, "har numrering inom serie"@sv, "has numbering within series"@en ;
    skos:definition "Met une manifestation en relation avec une indication d’ordre séquentiel d’une ou de plusieurs parties à l’intérieur d’une collection."@fr, "Relates a manifestation to a designation of the sequencing of a part or parts within a series."@en ;
    skos:scopeNote "La numérotation au sein d’une collection peut comprendre un chiffre, une lettre, tout autre caractère ou la combinaison de ces éléments, accompagnés ou non d’une appellation (volume, numéro, etc.) et/ou d’une indication chronologique."@fr, "Numbering includes a numeral, a letter, any other character, or the combination of these with or without an accompanying caption and/or a chronological designation."@en .

<http://rdaregistry.info/Elements/m/P30015>
    rdakit:instructionNumber "2.12.17" ;
    rdakit:toolkitDefinition "A designation of the sequencing of a part or parts within a subseries."@en, "Indication d’ordre séquentiel d’une ou de plusieurs parties à l’intérieur d’une sous-collection."@fr, "Una designación de la secuencia de una parte o partes dentro de la subserie."@es ;
    rdakit:toolkitLabel "numbering within subseries"@en, "numeración dentro de la subserie"@es, "numrering inom underserie"@sv, "numérotation au sein de la sous-collection"@fr ;
    reg:hasUnconstrained <http://rdaregistry.info/Elements/u/P60082> ;
    reg:lexicalAlias <http://rdaregistry.info/Elements/m/numberingWithinSubseries.en> ;
    reg:name "numberingWithinSubseries"@en ;
    reg:status <http://metadataregistry.org/uri/RegStatus/1001> ;
    a rdf:Property ;
    rdfs:domain <http://rdaregistry.info/Elements/c/C10007> ;
    rdfs:isDefinedBy <http://rdaregistry.info/Elements/m/> ;
    rdfs:label "a pour numérotation au sein de la sous-collection"@fr, "har numrering inom underserie"@sv, "has numbering within subseries"@en ;
    skos:definition "Met une manifestation en relation avec une indication d’ordre séquentiel d’une ou de plusieurs parties à l’intérieur d’une sous-collection."@fr, "Relates a manifestation to a designation of the sequencing of a part or parts within a subseries."@en ;
    skos:scopeNote "La numérotation au sein de la sous-collection peut comprendre un chiffre, une lettre, tout autre caractère ou la combinaison de ces éléments, accompagnés ou non d’une appellation (volume, numéro, etc.) et/ou d’une indication chronologique."@fr, "Numbering includes a numeral, a letter, any other character, or the combination of these with or without an accompanying caption and/or a chronological designation."@en .

<http://rdaregistry.info/Elements/m/P30016>
    rdakit:instructionNumber "24.5" ;
    rdakit:toolkitDefinition "A manifestation in a digital format that is the result of the transfer of a manifestation in an analog format."@en, "Manifestation en format numérique qui est le résultat du transfert d’une manifestation sur support analogique."@fr, "Una manifestación en un formato digital que es el resultado de la transferencia de una manifestación en un formato análogo."@es ;
    rdakit:toolkitLabel "electronic reproduction (manifestation)"@en, "reproducción electrónica (manifestación)"@es, "reproduction électronique (manifestation)"@fr ;
    reg:hasSubproperty <http://rdaregistry.info/Elements/m/object/P30016> ;
    reg:hasUnconstrained <http://rdaregistry.info/Elements/u/P60083> ;
    reg:lexicalAlias <http://rdaregistry.info/Elements/m/electronicReproductionManifestation.en> ;
    reg:name "electronicReproductionManifestation"@en ;
    reg:status <http://metadataregistry.org/uri/RegStatus/1001> ;
    a rdf:Property ;
    rdfs:domain <http://rdaregistry.info/Elements/c/C10007> ;
    rdfs:isDefinedBy <http://rdaregistry.info/Elements/m/> ;
    rdfs:label "a pour reproduction électronique (manifestation)"@fr, "has electronic reproduction (manifestation)"@en ;
    rdfs:subPropertyOf <http://rdaregistry.info/Elements/m/P30039> ;
    skos:definition "Met une manifestation en relation avec une manifestation en format numérique qui est le résultat du transfert d’une manifestation sur support analogique."@fr, "Relates a manifestation to a manifestation in a digital format that is the result of the transfer of a manifestation in an analog format."@en .

<http://rdaregistry.info/Elements/m/P30017>
    rdakit:instructionNumber "2.9.5" ;
    rdakit:toolkitDefinition "A distributor's name in a language or script that differs from that recorded in the distributor's name element."@en, "Nom de diffuseur ou de distributeur dans une langue et/ou une écriture différentes de celles enregistrées dans l’élément Nom de diffuseur ou de distributeur."@fr, "Un nombre de distribuidor en una lengua o escritura que difiere de la registrada en el elemento nombre del distribuidor."@es ;
    rdakit:toolkitLabel "forme parallèle du nom du diffuseur ou du distributeur"@fr, "nombre paralelo del distribuidor"@es, "parallel distributor's name"@en, "parallellt distributörsnamn"@sv ;
    reg:hasUnconstrained <http://rdaregistry.info/Elements/u/P60087> ;
    reg:lexicalAlias <http://rdaregistry.info/Elements/m/parallelDistributorsName.en> ;
    reg:name "parallelDistributorsName"@en ;
    reg:status <http://metadataregistry.org/uri/RegStatus/1001> ;
    a rdf:Property ;
    rdfs:domain <http://rdaregistry.info/Elements/c/C10007> ;
    rdfs:isDefinedBy <http://rdaregistry.info/Elements/m/> ;
    rdfs:label "a pour forme parallèle du nom du diffuseur ou du distributeur"@fr, "har parallellt distributörsnamn"@sv, "has parallel distributor’s name"@en ;
    skos:definition "Met une manifestation en relation avec un nom de diffuseur ou de distributeur dans une langue et/ou une écriture différentes de celles enregistrées dans l’élément Nom de diffuseur ou de distributeur."@fr, "Relates a manifestation to a distributor's name in a language or script that differs from that recorded in a distributor's name element."@en .

<http://rdaregistry.info/Elements/m/P30018>
    rdakit:instructionNumber "3.19.2" ;
    rdakit:toolkitDefinition "A general type of data content encoded in a computer file."@en, "Type général de contenu des données encodées dans un fichier informatique."@fr, "Un tipo general de contenido de datos codificado en un archivo de computadora."@es ;
    rdakit:toolkitLabel "file type"@en, "filtyp"@sv, "tipo de archivo"@es, "type de fichier"@fr ;
    reg:hasUnconstrained <http://rdaregistry.info/Elements/u/P60093> ;
    reg:lexicalAlias <http://rdaregistry.info/Elements/m/fileType.en> ;
    reg:name "fileType"@en ;
    reg:status <http://metadataregistry.org/uri/RegStatus/1001> ;
    a rdf:Property ;
    rdfs:domain <http://rdaregistry.info/Elements/c/C10007> ;
    rdfs:isDefinedBy <http://rdaregistry.info/Elements/m/> ;
    rdfs:label "a pour type de fichier"@fr, "har filtyp"@sv, "has file type"@en ;
    rdfs:subPropertyOf <http://rdaregistry.info/Elements/m/P30124> ;
    skos:definition "Met une manifestation en relation avec un type général de contenu des données encodées dans un fichier informatique."@fr, "Relates a manifestation to a general type of data content encoded in a computer file."@en .

<http://rdaregistry.info/Elements/m/P30019>
    rdakit:instructionNumber "24.5" ;
    rdakit:toolkitDefinition "A larger manifestation of which a part is a discrete component that exactly reproduces another manifestation embodying the same expression of a work."@en, "Manifestation plus vaste dont une partie est une composante distincte qui reproduit exactement une autre manifestation matérialisant la même expression d’une œuvre."@fr, "Una manifestación mayor de la cual una parte es un componente independiente que reproduce exactamente otra manifestación que materializa la misma expresión de una obra."@es ;
    rdakit:toolkitLabel "fac-similé contenu dans (manifestation)"@fr, "facsimile contained in"@en, "facsímil contenido en (manifestación)"@es ;
    reg:hasSubproperty <http://rdaregistry.info/Elements/m/object/P30019> ;
    reg:hasUnconstrained <http://rdaregistry.info/Elements/u/P60100> ;
    reg:lexicalAlias <http://rdaregistry.info/Elements/m/facsimileContainedIn.en> ;
    reg:name "facsimileContainedIn"@en ;
    reg:status <http://metadataregistry.org/uri/RegStatus/1001> ;
    a rdf:Property ;
    rdfs:domain <http://rdaregistry.info/Elements/c/C10007> ;
    rdfs:isDefinedBy <http://rdaregistry.info/Elements/m/> ;
    rdfs:label "est le fac-similé contenu dans (manifestation)"@fr, "is facsimile contained in"@en ;
    rdfs:subPropertyOf <http://rdaregistry.info/Elements/m/P30020> ;
    skos:definition "Met une manifestation en relation avec une manifestation plus vaste dont une partie est une composante distincte qui reproduit exactement une autre manifestation matérialisant la même expression d’une œuvre."@fr, "Relates a manifestation to a larger manifestation of which a part is a discrete component that exactly reproduces another manifestation embodying the same expression of a work."@en .

<http://rdaregistry.info/Elements/m/P30020>
    rdakit:instructionNumber "24.5" ;
    rdakit:toolkitDefinition "A larger manifestation of which the manifestation is a discrete component."@en, "Manifestation plus vaste dont la manifestation est une composante distincte."@fr, "Una manifestación mayor de la cual una parte es un componente separado."@es ;
    rdakit:toolkitLabel "contained in (manifestation)"@en, "contenida en (manifestación)"@es, "contenu dans (manifestation)"@fr ;
    reg:hasSubproperty <http://rdaregistry.info/Elements/m/P30019>, <http://rdaregistry.info/Elements/m/P30025>, <http://rdaregistry.info/Elements/m/P30101>, <http://rdaregistry.info/Elements/m/object/P30020> ;
    reg:hasUnconstrained <http://rdaregistry.info/Elements/u/P60101> ;
    reg:lexicalAlias <http://rdaregistry.info/Elements/m/containedInManifestation.en> ;
    reg:name "containedInManifestation"@en ;
    reg:status <http://metadataregistry.org/uri/RegStatus/1001> ;
    a rdf:Property ;
    rdfs:domain <http://rdaregistry.info/Elements/c/C10007> ;
    rdfs:isDefinedBy <http://rdaregistry.info/Elements/m/> ;
    rdfs:label "est contenu dans (manifestation)"@fr, "is contained in (manifestation)"@en ;
    rdfs:subPropertyOf <http://rdaregistry.info/Elements/m/P30213> ;
    skos:definition "Met une manifestation en relation avec une manifestation plus vaste dont la manifestation est une composante distincte."@fr, "Relates a manifestation to a larger manifestation of which the manifestation is a discrete component."@en .

<http://rdaregistry.info/Elements/m/P30021>
    rdakit:instructionNumber "24.5" ;
    rdakit:toolkitDefinition "A manifestation that consists of an exact reproduction on preservation-quality media, such as acid-free permanent or archival paper."@en, "Manifestation qui consiste en une reproduction exacte sur un support de qualité conservation, tel qu’un papier permanent sans acide ou un papier d’archivage."@fr, "Una manifestación que consiste en una reproducción exacta en un medio con calidad de preservación, tal como papel libre de ácido o papel de archivo."@es ;
    rdakit:toolkitLabel "fac-similé de conservation"@fr, "facsímil de preservación (manifestación)"@es, "preservation facsimile (manifestation)"@en ;
    reg:hasSubproperty <http://rdaregistry.info/Elements/m/object/P30021> ;
    reg:hasUnconstrained <http://rdaregistry.info/Elements/u/P60179> ;
    reg:lexicalAlias <http://rdaregistry.info/Elements/m/preservationFacsimileManifestation.en> ;
    reg:name "preservationFacsimileManifestation"@en ;
    reg:status <http://metadataregistry.org/uri/RegStatus/1001> ;
    a rdf:Property ;
    rdfs:domain <http://rdaregistry.info/Elements/c/C10007> ;
    rdfs:isDefinedBy <http://rdaregistry.info/Elements/m/> ;
    rdfs:label "a pour fac-similé de conservation"@fr, "has preservation facsimile (manifestation)"@en ;
    rdfs:subPropertyOf <http://rdaregistry.info/Elements/m/P30031> ;
    skos:definition "Met une manifestation en relation avec une manifestation qui consiste en une reproduction exacte sur un support de qualité conservation, tel qu’un papier permanent sans acide ou un papier d’archivage."@fr, "Relates a manifestation to a manifestation that consists of an exact reproduction on preservation-quality media, such as acid-free permanent or archival paper."@en .

<http://rdaregistry.info/Elements/m/P30022>
    rdakit:instructionNumber "24.5" ;
    rdakit:toolkitDefinition "A manifestation consisting of separately issued material that is not an integral part of a larger manifestation into which it has been inserted."@en, "Manifestation consistant en un document publié séparément qui ne fait pas partie intégrante de la manifestation plus vaste dans laquelle il a été encarté."@fr, "Una manifestación que consiste en material publicado separadamente, que no es parte integral de la manifestación mayor en la cual se inserta."@es ;
    rdakit:toolkitLabel "encart"@fr, "insert"@en, "inserto"@es ;
    reg:hasSubproperty <http://rdaregistry.info/Elements/m/object/P30022> ;
    reg:hasUnconstrained <http://rdaregistry.info/Elements/u/P60183> ;
    reg:lexicalAlias <http://rdaregistry.info/Elements/m/insert.en> ;
    reg:name "insert"@en ;
    reg:status <http://metadataregistry.org/uri/RegStatus/1001> ;
    a rdf:Property ;
    rdfs:domain <http://rdaregistry.info/Elements/c/C10007> ;
    rdfs:isDefinedBy <http://rdaregistry.info/Elements/m/> ;
    rdfs:label "est l’encart"@fr, "is insert"@en ;
    rdfs:subPropertyOf <http://rdaregistry.info/Elements/m/P30033> ;
    skos:definition "Met une manifestation en relation avec une manifestation consistant en un document publié séparément qui ne fait pas partie intégrante de la manifestation plus vaste dans laquelle il a été encarté."@fr, "Relates a manifestation to a manifestation consisting of separately issued material that is not an integral part of a larger manifestation into which it has been inserted."@en .

<http://rdaregistry.info/Elements/m/P30023>
    reg:status <http://metadataregistry.org/uri/RegStatus/1008> ;
    a rdf:Property ;
    rdfs:isDefinedBy <http://rdaregistry.info/Elements/m/> .

<http://rdaregistry.info/Elements/m/P30024>
    rdakit:instructionNumber "24.5" ;
    rdakit:toolkitDefinition "A manifestation that embodies the same expression of a work."@en, "Manifestation qui matérialise la même expression d’une œuvre."@fr, "Una manifestación que materializa la misma expresión de una obra."@es ;
    rdakit:toolkitLabel "equivalent (manifestation)"@en, "equivalente (manifestación)"@es, "équivalent (manifestation)"@fr ;
    reg:hasSubproperty <http://rdaregistry.info/Elements/m/P30026>, <http://rdaregistry.info/Elements/m/P30028>, <http://rdaregistry.info/Elements/m/P30039>, <http://rdaregistry.info/Elements/m/P30043>, <http://rdaregistry.info/Elements/m/object/P30024> ;
    reg:hasUnconstrained <http://rdaregistry.info/Elements/u/P60191> ;
    reg:lexicalAlias <http://rdaregistry.info/Elements/m/equivalentManifestation.en> ;
    reg:name "equivalentManifestation"@en ;
    reg:status <http://metadataregistry.org/uri/RegStatus/1001> ;
    a rdf:Property ;
    rdfs:domain <http://rdaregistry.info/Elements/c/C10007> ;
    rdfs:isDefinedBy <http://rdaregistry.info/Elements/m/> ;
    rdfs:label "est l’équivalent (manifestation)"@fr, "has equivalent (manifestation)"@en ;
    rdfs:subPropertyOf <http://rdaregistry.info/Elements/m/P30212> ;
    skos:definition "Met une manifestation en relation avec une manifestation qui matérialise la même expression d’une œuvre."@fr, "Relates a manifestation to a manifestation that embodies the same expression of a work."@en .

<http://rdaregistry.info/Elements/m/P30025>
    rdakit:instructionNumber "24.5" ;
    rdakit:toolkitDefinition "A manifestation into which material has been inserted that is not an integral part of the publication."@en, "Manifestation dans laquelle un document qui ne fait pas partie intégrante de la publication a été encarté."@fr, "Una manifestación en la cual se ha insertado material que no es parte integral de la publicación."@es ;
    rdakit:toolkitLabel "encarté dans"@fr, "insertada en"@es, "inserted in"@en ;
    reg:hasSubproperty <http://rdaregistry.info/Elements/m/object/P30025> ;
    reg:hasUnconstrained <http://rdaregistry.info/Elements/u/P60194> ;
    reg:lexicalAlias <http://rdaregistry.info/Elements/m/insertedIn.en> ;
    reg:name "insertedIn"@en ;
    reg:status <http://metadataregistry.org/uri/RegStatus/1001> ;
    a rdf:Property ;
    rdfs:domain <http://rdaregistry.info/Elements/c/C10007> ;
    rdfs:isDefinedBy <http://rdaregistry.info/Elements/m/> ;
    rdfs:label "est encarté dans"@fr, "is inserted in"@en ;
    rdfs:subPropertyOf <http://rdaregistry.info/Elements/m/P30020> ;
    skos:definition "Met une manifestation en relation avec une manifestation dans laquelle un document qui ne fait pas partie intégrante de la publication a été encarté."@fr, "Relates a manifestation to a manifestation into which material has been inserted that is not an integral part of the publication."@en .

<http://rdaregistry.info/Elements/m/P30026>
    rdakit:instructionNumber "24.5" ;
    rdakit:toolkitDefinition "A manifestation that embodies the same expression of a work in a different format."@en, "Manifestation matérialisant la même expression d’une œuvre sur un support différent."@fr, "Una manifestación que materializa la misma expresión de una obra en formato diferente."@es ;
    rdakit:toolkitLabel "also issued as"@en, "publicada también como"@es, "publié également comme"@fr ;
    reg:hasSubproperty <http://rdaregistry.info/Elements/m/object/P30026> ;
    reg:hasUnconstrained <http://rdaregistry.info/Elements/u/P60195> ;
    reg:lexicalAlias <http://rdaregistry.info/Elements/m/alsoIssuedAs.en> ;
    reg:name "alsoIssuedAs"@en ;
    reg:status <http://metadataregistry.org/uri/RegStatus/1001> ;
    a rdf:Property ;
    rdfs:domain <http://rdaregistry.info/Elements/c/C10007> ;
    rdfs:isDefinedBy <http://rdaregistry.info/Elements/m/> ;
    rdfs:label "est publié également comme"@fr, "is also issued as"@en ;
    rdfs:subPropertyOf <http://rdaregistry.info/Elements/m/P30024> ;
    skos:definition "Met une manifestation en relation avec une manifestation matérialisant la même expression d’une œuvre sur un support différent."@fr, "Relates a manifestation to a manifestation that embodies the same expression of a work in a different format."@en .

<http://rdaregistry.info/Elements/m/P30027>
    rdakit:instructionNumber "24.5" ;
    rdakit:toolkitDefinition "A manifestation issued with another manifestation, without any relationship to its content."@en, "Manifestation publiée avec une autre manifestation, sans aucune relation avec son contenu."@fr, "Una manifestación publicada con otra manifestación, sin ninguna relación con su contenido."@es ;
    rdakit:toolkitLabel "accompagné de (manifestation)"@fr, "accompanied by (manifestation)"@en, "acompañado por (manifestación)"@es ;
    reg:hasSubproperty <http://rdaregistry.info/Elements/m/P30035>, <http://rdaregistry.info/Elements/m/object/P30027> ;
    reg:hasUnconstrained <http://rdaregistry.info/Elements/u/P60196> ;
    reg:lexicalAlias <http://rdaregistry.info/Elements/m/accompaniedByManifestation.en> ;
    reg:name "accompaniedByManifestation"@en ;
    reg:status <http://metadataregistry.org/uri/RegStatus/1001> ;
    a rdf:Property ;
    rdfs:domain <http://rdaregistry.info/Elements/c/C10007> ;
    rdfs:isDefinedBy <http://rdaregistry.info/Elements/m/> ;
    rdfs:label "est accompagné de (manifestation)"@fr, "is accompanied by (manifestation)"@en ;
    rdfs:subPropertyOf <http://rdaregistry.info/Elements/m/P30210> ;
    skos:definition "Met une manifestation en relation avec une manifestation publiée avec une autre manifestation, sans aucune relation avec son contenu."@fr, "Relates a manifestation to a manifestation issued with another manifestation, without any relationship to its content."@en .

<http://rdaregistry.info/Elements/m/P30028>
    rdakit:instructionNumber "24.5" ;
    rdakit:toolkitDefinition "A manifestation that is an exact copy of a website, used to reduce network traffic or improve the availability of the content of the original site."@en, "Manifestation qui est une copie exacte d’un site Web, utilisée pour réduire le trafic sur le réseau ou augmenter la disponibilité du contenu du site d’origine."@fr, "Una manifestación que es una copia exacta de un sitio web, usada para reducir el tráfico en la red o mejorar la disponibilidad del sitio original."@es ;
    rdakit:toolkitLabel "mirror site"@en, "site miroir"@fr, "sitio espejo"@es ;
    reg:hasSubproperty <http://rdaregistry.info/Elements/m/object/P30028> ;
    reg:hasUnconstrained <http://rdaregistry.info/Elements/u/P60197> ;
    reg:lexicalAlias <http://rdaregistry.info/Elements/m/mirrorSite.en> ;
    reg:name "mirrorSite"@en ;
    reg:status <http://metadataregistry.org/uri/RegStatus/1001> ;
    a rdf:Property ;
    rdfs:domain <http://rdaregistry.info/Elements/c/C10007> ;
    rdfs:isDefinedBy <http://rdaregistry.info/Elements/m/> ;
    rdfs:label "est le site miroir"@fr, "is mirror site"@en ;
    rdfs:subPropertyOf <http://rdaregistry.info/Elements/m/P30024> ;
    skos:definition "Met une manifestation en relation avec une manifestation qui est une copie exacte d’un site Web, utilisée pour réduire le trafic sur le réseau ou augmenter la disponibilité du contenu du site d’origine."@fr, "Relates a manifestation to a manifestation that is an exact copy of a website, used to reduce network traffic or improve the availability of the content of the original site."@en .

<http://rdaregistry.info/Elements/m/P30029>
    rdakit:instructionNumber "24.5" ;
    rdakit:toolkitDefinition "A manifestation in a digital format that results from the transfer of a manifestation in another digital format."@en, "Manifestation en format numérique qui résulte du transfert d’une manifestation dans un format numérique différent."@fr, "Una manifestación en formato digital que resulta de la transferencia de una manifestación en otro formato digital."@es ;
    rdakit:toolkitLabel "digital transfer (manifestation)"@en, "transferencia digital (manifestación)"@es, "transfert numérique (manifestation)"@fr ;
    reg:hasSubproperty <http://rdaregistry.info/Elements/m/object/P30029> ;
    reg:hasUnconstrained <http://rdaregistry.info/Elements/u/P60200> ;
    reg:lexicalAlias <http://rdaregistry.info/Elements/m/digitalTransferManifestation.en> ;
    reg:name "digitalTransferManifestation"@en ;
    reg:status <http://metadataregistry.org/uri/RegStatus/1001> ;
    a rdf:Property ;
    rdfs:domain <http://rdaregistry.info/Elements/c/C10007> ;
    rdfs:isDefinedBy <http://rdaregistry.info/Elements/m/> ;
    rdfs:label "a pour transfert numérique (manifestation)"@fr, "has digital transfer (manifestation)"@en ;
    rdfs:subPropertyOf <http://rdaregistry.info/Elements/m/P30039> ;
    skos:definition "Met une manifestation en relation avec une manifestation en format numérique qui résulte du transfert d’une manifestation dans un format numérique différent."@fr, "Relates a manifestation to a manifestation in a digital format that results from the transfer of a manifestation in another digital format."@en .

<http://rdaregistry.info/Elements/m/P30030>
    rdakit:instructionNumber "24.5" ;
    rdakit:toolkitDefinition "A manifestation that consists of a single issue or a supplementary section of a periodical or newspaper devoted to a special subject, with or without serial numbering."@en, "Manifestation qui consiste en un numéro isolé ou un supplément d’une publication en série ou d’un journal consacré à un sujet spécifique."@fr, "Una manifestación que contiene un número o sección suplementaria de una publicación seriada o periódico dedicada a un tema especial."@es ;
    rdakit:toolkitLabel "numéro spécial"@fr, "número especial"@es, "special issue"@en ;
    reg:hasSubproperty <http://rdaregistry.info/Elements/m/object/P30030> ;
    reg:hasUnconstrained <http://rdaregistry.info/Elements/u/P60207> ;
    reg:lexicalAlias <http://rdaregistry.info/Elements/m/specialIssue.en> ;
    reg:name "specialIssue"@en ;
    reg:status <http://metadataregistry.org/uri/RegStatus/1001> ;
    a rdf:Property ;
    rdfs:domain <http://rdaregistry.info/Elements/c/C10007> ;
    rdfs:isDefinedBy <http://rdaregistry.info/Elements/m/> ;
    rdfs:label "est le numéro spécial"@fr, "is special issue"@en ;
    rdfs:subPropertyOf <http://rdaregistry.info/Elements/m/P30033> ;
    skos:definition "Met une manifestation en relation avec une manifestation qui consiste en un numéro isolé ou un supplément d’une publication en série ou d’un journal consacré à un sujet spécifique."@fr, "Relates a manifestation to a manifestation that consists of a single issue or a supplementary section of a periodical or newspaper devoted to a special subject, with or without serial numbering."@en .

<http://rdaregistry.info/Elements/m/P30031>
    rdakit:instructionNumber "24.5" ;
    rdakit:toolkitDefinition "A manifestation that exactly reproduces another manifestation."@en, "Manifestation qui reproduit exactement une autre manifestation."@fr, "Una manifestación que reproduce exactamente otra manifestación."@es ;
    rdakit:toolkitLabel "fac-similé (manifestation)"@fr, "facsimile (manifestation)"@en, "facsímil (manifestación)"@es ;
    reg:hasSubproperty <http://rdaregistry.info/Elements/m/P30021>, <http://rdaregistry.info/Elements/m/object/P30031> ;
    reg:hasUnconstrained <http://rdaregistry.info/Elements/u/P60217> ;
    reg:lexicalAlias <http://rdaregistry.info/Elements/m/facsimileManifestation.en> ;
    reg:name "facsimileManifestation"@en ;
    reg:status <http://metadataregistry.org/uri/RegStatus/1001> ;
    a rdf:Property ;
    rdfs:domain <http://rdaregistry.info/Elements/c/C10007> ;
    rdfs:isDefinedBy <http://rdaregistry.info/Elements/m/> ;
    rdfs:label "a pour fac-similé (manifestation)"@fr, "has facsimile (manifestation)"@en ;
    rdfs:subPropertyOf <http://rdaregistry.info/Elements/m/P30039> ;
    skos:definition "Met une manifestation en relation avec une manifestation qui reproduit exactement une autre manifestation."@fr, "Relates a manifestation to a manifestation that exactly reproduces another manifestation."@en .

<http://rdaregistry.info/Elements/m/P30032>
    reg:status <http://metadataregistry.org/uri/RegStatus/1008> ;
    a rdf:Property ;
    rdfs:isDefinedBy <http://rdaregistry.info/Elements/m/> .

<http://rdaregistry.info/Elements/m/P30033>
    rdakit:instructionNumber "24.5" ;
    rdakit:toolkitDefinition "A manifestation that is a discrete component of a larger manifestation."@en, "Manifestation qui est une composante distincte d’une manifestation plus vaste."@fr, "Una manifestación que es un componente separado de una entidad mayor."@es ;
    rdakit:toolkitLabel "container of (manifestation)"@en, "conteneur de (manifestation)"@fr, "contiene (manifestación)"@es ;
    reg:hasSubproperty <http://rdaregistry.info/Elements/m/P30022>, <http://rdaregistry.info/Elements/m/P30030>, <http://rdaregistry.info/Elements/m/P30046>, <http://rdaregistry.info/Elements/m/object/P30033> ;
    reg:hasUnconstrained <http://rdaregistry.info/Elements/u/P60249> ;
    reg:lexicalAlias <http://rdaregistry.info/Elements/m/containerOfManifestation.en> ;
    reg:name "containerOfManifestation"@en ;
    reg:status <http://metadataregistry.org/uri/RegStatus/1001> ;
    a rdf:Property ;
    rdfs:domain <http://rdaregistry.info/Elements/c/C10007> ;
    rdfs:isDefinedBy <http://rdaregistry.info/Elements/m/> ;
    rdfs:label "est le conteneur de (manifestation)"@fr, "is container of (manifestation)"@en ;
    rdfs:subPropertyOf <http://rdaregistry.info/Elements/m/P30213> ;
    skos:definition "Met une manifestation en relation avec une manifestation qui est une composante distincte d’une manifestation plus vaste."@fr, "Relates a manifestation to a manifestation that is a discrete component of a larger manifestation."@en .

<http://rdaregistry.info/Elements/m/P30034>
    reg:status <http://metadataregistry.org/uri/RegStatus/1008> ;
    a rdf:Property ;
    rdfs:isDefinedBy <http://rdaregistry.info/Elements/m/> .

<http://rdaregistry.info/Elements/m/P30035>
    rdakit:instructionNumber "24.5" ;
    rdakit:toolkitDefinition "A manifestation that is issued on the same carrier as a manifestation being described."@en, "Manifestation qui est publiée sur le même support matériel que la manifestation décrite."@fr, "Una manifestación que se publica en el mismo soporte que la manifestación que se está describiendo."@es ;
    rdakit:toolkitLabel "issued with"@en, "publicado con"@es, "publié avec"@fr ;
    reg:hasSubproperty <http://rdaregistry.info/Elements/m/P30036>, <http://rdaregistry.info/Elements/m/P30037>, <http://rdaregistry.info/Elements/m/object/P30035> ;
    reg:hasUnconstrained <http://rdaregistry.info/Elements/u/P60256> ;
    reg:lexicalAlias <http://rdaregistry.info/Elements/m/issuedWith.en> ;
    reg:name "issuedWith"@en ;
    reg:status <http://metadataregistry.org/uri/RegStatus/1001> ;
    a rdf:Property ;
    rdfs:domain <http://rdaregistry.info/Elements/c/C10007> ;
    rdfs:isDefinedBy <http://rdaregistry.info/Elements/m/> ;
    rdfs:label "est publié avec"@fr, "is issued with"@en ;
    rdfs:subPropertyOf <http://rdaregistry.info/Elements/m/P30027> ;
    skos:definition "Met une manifestation en relation avec une manifestation qui est publiée sur le même support matériel que la manifestation décrite."@fr, "Relates a manifestation to a manifestation that is issued on the same carrier as a manifestation being described."@en .

<http://rdaregistry.info/Elements/m/P30036>
    rdakit:instructionNumber "24.5" ;
    rdakit:toolkitDefinition "A manifestation that is issued on the same disc with a manifestation being described."@en, "Manifestation qui est publiée sur le même disque que la manifestation décrite."@fr, "Una manifestación que está publicada en el mismo disco que la manifestación que se está describiendo."@es ;
    rdakit:toolkitLabel "en disco con (manifestación)"@es, "on disc with (manifestation)"@en, "sur le disque avec (manifestation)"@fr ;
    reg:hasSubproperty <http://rdaregistry.info/Elements/m/object/P30036> ;
    reg:hasUnconstrained <http://rdaregistry.info/Elements/u/P60257> ;
    reg:lexicalAlias <http://rdaregistry.info/Elements/m/onDiscWithManifestation.en> ;
    reg:name "onDiscWithManifestation"@en ;
    reg:status <http://metadataregistry.org/uri/RegStatus/1001> ;
    a rdf:Property ;
    rdfs:domain <http://rdaregistry.info/Elements/c/C10007> ;
    rdfs:isDefinedBy <http://rdaregistry.info/Elements/m/> ;
    rdfs:label "est sur le disque avec (manifestation)"@fr, "is on disc with (manifestation)"@en ;
    rdfs:subPropertyOf <http://rdaregistry.info/Elements/m/P30035> ;
    skos:definition "Met une manifestation en relation avec une manifestation qui est publiée sur le même disque que la manifestation décrite."@fr, "Relates a manifestation to a manifestation that is issued on the same disc with a manifestation being described."@en .

<http://rdaregistry.info/Elements/m/P30037>
    rdakit:instructionNumber "24.5" ;
    rdakit:toolkitDefinition "A manifestation that is issued on the same microform with a manifestation being described."@en, "Manifestation qui est publiée sur la même microforme que la manifestation décrite."@fr, "Una manifestación que está publicada en la misma microforma que la manifestación que se está describiendo."@es ;
    rdakit:toolkitLabel "filmada con (manifestación)"@es, "filmed with (manifestation)"@en, "filmé avec (manifestation)"@fr ;
    reg:hasSubproperty <http://rdaregistry.info/Elements/m/object/P30037> ;
    reg:hasUnconstrained <http://rdaregistry.info/Elements/u/P60258> ;
    reg:lexicalAlias <http://rdaregistry.info/Elements/m/filmedWithManifestation.en> ;
    reg:name "filmedWithManifestation"@en ;
    reg:status <http://metadataregistry.org/uri/RegStatus/1001> ;
    a rdf:Property ;
    rdfs:domain <http://rdaregistry.info/Elements/c/C10007> ;
    rdfs:isDefinedBy <http://rdaregistry.info/Elements/m/> ;
    rdfs:label "est filmé avec (manifestation)"@fr, "is filmed with (manifestation)"@en ;
    rdfs:subPropertyOf <http://rdaregistry.info/Elements/m/P30035> ;
    skos:definition "Met une manifestation en relation avec une manifestation qui est publiée sur la même microforme que la manifestation décrite."@fr, "Relates a manifestation to a manifestation that is issued on the same microform with a manifestation being described."@en .

<http://rdaregistry.info/Elements/m/P30038>
    rdakit:instructionNumber "24.5" ;
    rdakit:toolkitDefinition "A manifestation that is a reissue of another printed manifestation."@en, "Manifestation qui est une réédition d’une autre manifestation imprimée."@fr, "Una manifestación que es una reedición de otra manifestación impresa."@es ;
    rdakit:toolkitLabel "reimpreso como (manifestación)"@es, "reprinted as (manifestation)"@en, "réimprimé comme (manifestation)"@fr ;
    reg:hasSubproperty <http://rdaregistry.info/Elements/m/object/P30038> ;
    reg:hasUnconstrained <http://rdaregistry.info/Elements/u/P60271> ;
    reg:lexicalAlias <http://rdaregistry.info/Elements/m/reprintedAsManifestation.en> ;
    reg:name "reprintedAsManifestation"@en ;
    reg:status <http://metadataregistry.org/uri/RegStatus/1001> ;
    a rdf:Property ;
    rdfs:domain <http://rdaregistry.info/Elements/c/C10007> ;
    rdfs:isDefinedBy <http://rdaregistry.info/Elements/m/> ;
    rdfs:label "est réimprimé comme (manifestation)"@fr, "is reprinted as (manifestation)"@en ;
    rdfs:subPropertyOf <http://rdaregistry.info/Elements/m/P30039> ;
    skos:definition "Met une manifestation en relation avec une manifestation qui est une réédition d’une autre manifestation imprimée."@fr, "Relates a manifestation to a manifestation that is a reissue of another printed manifestation."@en .

<http://rdaregistry.info/Elements/m/P30039>
    rdakit:instructionNumber "24.5" ;
    rdakit:toolkitDefinition "A manifestation that reproduces another manifestation."@en, "Manifestation qui reproduit une autre manifestation."@fr, "Una manifestación que reproduce otra manifestación."@es ;
    rdakit:toolkitLabel "reproduced as (manifestation)"@en, "reproducida como (manifestación)"@es, "reproduit comme (manifestation)"@fr ;
    reg:hasSubproperty <http://rdaregistry.info/Elements/m/P30016>, <http://rdaregistry.info/Elements/m/P30029>, <http://rdaregistry.info/Elements/m/P30031>, <http://rdaregistry.info/Elements/m/P30038>, <http://rdaregistry.info/Elements/m/object/P30039> ;
    reg:hasUnconstrained <http://rdaregistry.info/Elements/u/P60272> ;
    reg:lexicalAlias <http://rdaregistry.info/Elements/m/reproducedAsManifestation.en> ;
    reg:name "reproducedAsManifestation"@en ;
    reg:status <http://metadataregistry.org/uri/RegStatus/1001> ;
    a rdf:Property ;
    rdfs:domain <http://rdaregistry.info/Elements/c/C10007> ;
    rdfs:isDefinedBy <http://rdaregistry.info/Elements/m/> ;
    rdfs:label "est reproduit comme (manifestation)"@fr, "is reproduced as (manifestation)"@en ;
    rdfs:subPropertyOf <http://rdaregistry.info/Elements/m/P30024> ;
    skos:definition "Met une manifestation en relation avec une manifestation qui reproduit une autre manifestation."@fr, "Relates a manifestation to a manifestation that reproduces another manifestation."@en .

<http://rdaregistry.info/Elements/m/P30040>
    rdakit:instructionNumber "24.5" ;
    rdakit:toolkitDefinition "A manifestation in a digital format that is transferred to another digital format."@en, "Manifestation en format numérique qui a été transférée dans un format numérique différent."@fr, "Una manifestación en un formato digital que se transfiere a otro formato digital."@es ;
    rdakit:toolkitLabel "digital transfer of (manifestation)"@en, "transferencia digital de (manifestación)"@es, "transfert numérique de (manifestation)"@fr ;
    reg:hasSubproperty <http://rdaregistry.info/Elements/m/object/P30040> ;
    reg:hasUnconstrained <http://rdaregistry.info/Elements/u/P60287> ;
    reg:lexicalAlias <http://rdaregistry.info/Elements/m/digitalTransferOfManifestation.en> ;
    reg:name "digitalTransferOfManifestation"@en ;
    reg:status <http://metadataregistry.org/uri/RegStatus/1001> ;
    a rdf:Property ;
    rdfs:domain <http://rdaregistry.info/Elements/c/C10007> ;
    rdfs:isDefinedBy <http://rdaregistry.info/Elements/m/> ;
    rdfs:label "est le transfert numérique de (manifestation)"@fr, "is digital transfer of (manifestation)"@en ;
    rdfs:subPropertyOf <http://rdaregistry.info/Elements/m/P30043> ;
    skos:definition "Met une manifestation en relation avec une manifestation en format numérique qui a été transférée dans un format numérique différent."@fr, "Relates a manifestation to a manifestation in a digital format that is transferred to another digital format."@en .

<http://rdaregistry.info/Elements/m/P30041>
    reg:status <http://metadataregistry.org/uri/RegStatus/1008> ;
    a rdf:Property ;
    rdfs:isDefinedBy <http://rdaregistry.info/Elements/m/> .

<http://rdaregistry.info/Elements/m/P30042>
    reg:status <http://metadataregistry.org/uri/RegStatus/1008> ;
    a rdf:Property ;
    rdfs:isDefinedBy <http://rdaregistry.info/Elements/m/> .

<http://rdaregistry.info/Elements/m/P30043>
    rdakit:instructionNumber "24.5" ;
    rdakit:toolkitDefinition "A manifestation that is used as the basis for a reproduction."@en, "Manifestation servant de base à une reproduction."@fr, "Una manifestación utilizada como base para una reproducción."@es ;
    rdakit:toolkitLabel "reproducción de (manifestación)"@es, "reproduction de (manifestation)"@fr, "reproduction of (manifestation)"@en ;
    reg:hasSubproperty <http://rdaregistry.info/Elements/m/P30040>, <http://rdaregistry.info/Elements/m/P30047>, <http://rdaregistry.info/Elements/m/P30093>, <http://rdaregistry.info/Elements/m/P30136>, <http://rdaregistry.info/Elements/m/object/P30043> ;
    reg:hasUnconstrained <http://rdaregistry.info/Elements/u/P60297> ;
    reg:lexicalAlias <http://rdaregistry.info/Elements/m/reproductionOfManifestation.en> ;
    reg:name "reproductionOfManifestation"@en ;
    reg:status <http://metadataregistry.org/uri/RegStatus/1001> ;
    a rdf:Property ;
    rdfs:domain <http://rdaregistry.info/Elements/c/C10007> ;
    rdfs:isDefinedBy <http://rdaregistry.info/Elements/m/> ;
    rdfs:label "est la reproduction de (manifestation)"@fr, "is reproduction of (manifestation)"@en ;
    rdfs:subPropertyOf <http://rdaregistry.info/Elements/m/P30024> ;
    skos:definition "Met une manifestation en relation avec une manifestation servant de base à une reproduction."@fr, "Relates a manifestation to a manifestation that is used as the basis for a reproduction."@en .

<http://rdaregistry.info/Elements/m/P30044>
    reg:status <http://metadataregistry.org/uri/RegStatus/1008> ;
    a rdf:Property ;
    rdfs:isDefinedBy <http://rdaregistry.info/Elements/m/> .

<http://rdaregistry.info/Elements/m/P30045>
    rdakit:instructionNumber "24.5" ;
    rdakit:toolkitDefinition "A manifestation that is used as the basis for an exact reproduction on preservation-quality media, such as acid-free permanent or archival paper."@en, "Manifestation servant de base à une reproduction exacte sur un support de qualité conservation, tel qu’un papier permanent sans acide ou un papier d’archivage."@fr, "Una manifestación utilizada como base para una reproducción exacta sobre un medio con calidad de preservación, tal como papel libre de ácido o papel de archivo."@es ;
    rdakit:toolkitLabel "fac-similé de conservation de (manifestation)"@fr, "facsímil de preservación de (manifestación)"@es, "preservation facsimile of (manifestation)"@en ;
    reg:hasSubproperty <http://rdaregistry.info/Elements/m/object/P30045> ;
    reg:hasUnconstrained <http://rdaregistry.info/Elements/u/P60299> ;
    reg:lexicalAlias <http://rdaregistry.info/Elements/m/preservationFacsimileOfManifestation.en> ;
    reg:name "preservationFacsimileOfManifestation"@en ;
    reg:status <http://metadataregistry.org/uri/RegStatus/1001> ;
    a rdf:Property ;
    rdfs:domain <http://rdaregistry.info/Elements/c/C10007> ;
    rdfs:isDefinedBy <http://rdaregistry.info/Elements/m/> ;
    rdfs:label "est le fac-similé de conservation de (manifestation)"@fr, "is preservation facsimile of (manifestation)"@en ;
    rdfs:subPropertyOf <http://rdaregistry.info/Elements/m/P30047> ;
    skos:definition "Met une manifestation en relation avec une manifestation servant de base à une reproduction exacte sur un support de qualité conservation, tel qu’un papier permanent sans acide ou un papier d’archivage."@fr, "Relates a manifestation to a manifestation that is used as the basis for an exact reproduction on preservation-quality media, such as acid-free permanent or archival paper."@en .

<http://rdaregistry.info/Elements/m/P30046>
    rdakit:instructionNumber "24.5" ;
    rdakit:toolkitDefinition "A manifestation used as the basis for an exact reproduction that is a discrete component of a larger manifestation."@en, "Manifestation servant de base à une reproduction exacte qui est une composante distincte d’une manifestation plus vaste."@fr, "Una manifestación utilizada como base para una reproducción exacta que es un componente individual de una entidad mayor."@es ;
    rdakit:toolkitLabel "conteneur fac-similé de (manifestation)"@fr, "contiene facsímil de (manifestación)"@es, "facsimile container of"@en ;
    reg:hasSubproperty <http://rdaregistry.info/Elements/m/object/P30046> ;
    reg:hasUnconstrained <http://rdaregistry.info/Elements/u/P60300> ;
    reg:lexicalAlias <http://rdaregistry.info/Elements/m/facsimileContainerOf.en> ;
    reg:name "facsimileContainerOf"@en ;
    reg:status <http://metadataregistry.org/uri/RegStatus/1001> ;
    a rdf:Property ;
    rdfs:domain <http://rdaregistry.info/Elements/c/C10007> ;
    rdfs:isDefinedBy <http://rdaregistry.info/Elements/m/> ;
    rdfs:label "est le conteneur fac-similé de (manifestation)"@fr, "is facsimile container of"@en ;
    rdfs:subPropertyOf <http://rdaregistry.info/Elements/m/P30033> ;
    skos:definition "Met une manifestation en relation avec une manifestation servant de base à une reproduction exacte qui est une composante distincte d’une manifestation plus vaste."@fr, "Relates a manifestation to a manifestation used as the basis for an exact reproduction that is a discrete component of a larger manifestation."@en .

<http://rdaregistry.info/Elements/m/P30047>
    rdakit:instructionNumber "24.5" ;
    rdakit:toolkitDefinition "A manifestation that is used as the basis for an exact reproduction."@en, "Manifestation servant de base à une reproduction exacte."@fr, "Una manifestación usada como base para un reproducción exacta."@es ;
    rdakit:toolkitLabel "fac-similé de (manifestation)"@fr, "facsimile of (manifestation)"@en, "facsímil de (manifestación)"@es ;
    reg:hasSubproperty <http://rdaregistry.info/Elements/m/P30045>, <http://rdaregistry.info/Elements/m/object/P30047> ;
    reg:hasUnconstrained <http://rdaregistry.info/Elements/u/P60301> ;
    reg:lexicalAlias <http://rdaregistry.info/Elements/m/facsimileOfManifestation.en> ;
    reg:name "facsimileOfManifestation"@en ;
    reg:status <http://metadataregistry.org/uri/RegStatus/1001> ;
    a rdf:Property ;
    rdfs:domain <http://rdaregistry.info/Elements/c/C10007> ;
    rdfs:isDefinedBy <http://rdaregistry.info/Elements/m/> ;
    rdfs:label "est le fac-similé de (manifestation)"@fr, "is facsimile of (manifestation)"@en ;
    rdfs:subPropertyOf <http://rdaregistry.info/Elements/m/P30043> ;
    skos:definition "Met une manifestation en relation avec une manifestation servant de base à une reproduction exacte."@fr, "Relates a manifestation to a manifestation that is used as the basis for an exact reproduction."@en .

<http://rdaregistry.info/Elements/m/P30048>
    rdakit:toolkitLabel "relaterad manifestation"@sv ;
    reg:hasSubproperty <http://rdaregistry.info/Elements/m/P30210>, <http://rdaregistry.info/Elements/m/P30212>, <http://rdaregistry.info/Elements/m/P30213>, <http://rdaregistry.info/Elements/m/datatype/P30048>, <http://rdaregistry.info/Elements/m/object/P30048> ;
    reg:hasUnconstrained <http://rdaregistry.info/Elements/u/P60313> ;
    reg:lexicalAlias <http://rdaregistry.info/Elements/m/relatedManifestationManifestation.en> ;
    reg:name "relatedManifestationManifestation"@en ;
    reg:status <http://metadataregistry.org/uri/RegStatus/1001> ;
    a rdf:Property ;
    rdfs:domain <http://rdaregistry.info/Elements/c/C10007> ;
    rdfs:isDefinedBy <http://rdaregistry.info/Elements/m/> ;
    rdfs:label "har relaterad manifestation"@sv, "has related manifestation (manifestation)"@en ;
    rdfs:subPropertyOf <http://rdaregistry.info/Elements/m/P30264> ;
    skos:definition "Relates a manifestation to a manifestation associated with a manifestation being described."@en .

<http://rdaregistry.info/Elements/m/P30049>
    rdakit:instructionNumber "2.10.5" ;
    rdakit:toolkitDefinition "A manufacturer's name in a language or script that differs from that recorded in a manufacturer's name element."@en, "Nom de fabricant dans une langue et/ou une écriture différentes de celles enregistrées dans l’élément Nom de fabricant."@fr, "Un nombre del fabricante en una lengua y/o escritura que difiere de la registrada en el elemento nombre del fabricante."@es ;
    rdakit:toolkitLabel "forme parallèle du nom du fabricant"@fr, "nombre paralelo del fabricante"@es, "parallel manufacturer's name"@en, "parallellt tillverkningsnamn"@sv ;
    reg:hasUnconstrained <http://rdaregistry.info/Elements/u/P60108> ;
    reg:lexicalAlias <http://rdaregistry.info/Elements/m/parallelManufacturersName.en> ;
    reg:name "parallelManufacturersName"@en ;
    reg:status <http://metadataregistry.org/uri/RegStatus/1001> ;
    a rdf:Property ;
    rdfs:domain <http://rdaregistry.info/Elements/c/C10007> ;
    rdfs:isDefinedBy <http://rdaregistry.info/Elements/m/> ;
    rdfs:label "a pour forme parallèle du nom du fabricant"@fr, "har parallellt tillverkningsnamn"@sv, "has parallel manufacturer’s name"@en ;
    skos:definition "Met une manifestation en relation avec un nom de fabricant dans une langue et/ou une écriture différentes de celles enregistrées dans l’élément Nom de fabricant."@fr, "Relates a manifestation to a manufacturer's name in a language or script that differs from that recorded in a manufacturer's name element."@en .

<http://rdaregistry.info/Elements/m/P30050>
    rdakit:instructionNumber "2.17.13" ;
    rdakit:toolkitDefinition "A note identifying an issue or part of a multipart monograph or serial, or an iteration of an integrating resource that has been used as a basis for the identification of a manifestation."@en, "Note identifiant la livraison d’une publication en série ou la partie d’une monographie en plusieurs parties ou bien l’itération d’une ressource intégratrice qui a servi de base pour l’identification d’une ressource."@fr, "Una nota que identifica la entrega o parte de una monografía en varias partes o publicación seriada, o la iteración de un recurso integrado que se ha utilizado como base para la identificación de un recurso."@es ;
    rdakit:toolkitLabel "anmärkning om nummer, del eller uppdatering som beskrivningen grundar sig på"@sv, "nota sobre entrega, parte o iteración usada como base para la identificación del recurso"@es, "note on issue, part, or iteration used as basis for identification of manifestation"@en, "note relative à la livraison, la partie ou l’itération servant de base pour l’identification de la ressource"@fr ;
    reg:hasUnconstrained <http://rdaregistry.info/Elements/u/P60122> ;
    reg:lexicalAlias <http://rdaregistry.info/Elements/m/noteOnIssuePartOrIterationUsedAsBasisForIdentificationOfManifestation.en> ;
    reg:name "noteOnIssuePartOrIterationUsedAsBasisForIdentificationOfManifestation"@en ;
    reg:status <http://metadataregistry.org/uri/RegStatus/1001> ;
    a rdf:Property ;
    rdfs:domain <http://rdaregistry.info/Elements/c/C10007> ;
    rdfs:isDefinedBy <http://rdaregistry.info/Elements/m/> ;
    rdfs:label "a pour note relative à la livraison, la partie ou l’itération servant de base pour l’identification de la ressource"@fr, "har anmärkning om nummer, del eller uppdatering som beskrivningen grundar sig på"@sv, "has note on issue, part, or iteration used as basis for identification of manifestation"@en ;
    rdfs:subPropertyOf <http://rdaregistry.info/Elements/m/P30137> ;
    skos:definition "Met une manifestation en relation avec une note identifiant la livraison d’une publication en série ou la partie d’une monographie en plusieurs parties ou bien l’itération d’une ressource intégratrice qui a servi de base pour l’identification d’une ressource."@fr, "Relates a manifestation to a note identifying an issue or part of a multipart monograph or serial, or an iteration of an integrating resource that has been used as a basis for the identification of a manifestation."@en .

<http://rdaregistry.info/Elements/m/P30051>
    rdakit:instructionNumber "3.21.4" ;
    rdakit:toolkitDefinition "A note on changes in the characteristics of the carrier that occur in subsequent issues or parts of a manifestation issued in successive parts or between iterations of an integrating resource."@en, "Note portant sur les changements dans les caractéristiques du support matériel survenant dans les livraisons ou parties ultérieures d’une ressource publiée en parties successives ou bien entre les différentes itérations d’une ressource intégratrice."@fr, "Una nota sobre cambios en las características del soporte que ocurren en entregas o partes subsecuentes del recurso publicado en partes sucesivas o entre iteraciones de un recurso integrado."@es ;
    rdakit:toolkitLabel "anmärkning om förändringar i bäraregenskaper"@sv, "nota sobre los cambios en las características del soporte"@es, "note on changes in carrier characteristics"@en, "note sur les changements dans les caractéristiques du support matériel"@fr ;
    reg:hasUnconstrained <http://rdaregistry.info/Elements/u/P60124> ;
    reg:lexicalAlias <http://rdaregistry.info/Elements/m/noteOnChangesInCarrierCharacteristics.en> ;
    reg:name "noteOnChangesInCarrierCharacteristics"@en ;
    reg:status <http://metadataregistry.org/uri/RegStatus/1001> ;
    a rdf:Property ;
    rdfs:domain <http://rdaregistry.info/Elements/c/C10007> ;
    rdfs:isDefinedBy <http://rdaregistry.info/Elements/m/> ;
    rdfs:label "a pour note sur les changements dans les caractéristiques du support matériel"@fr, "har anmärkning om förändringar i bäraregenskaper"@sv, "has note on changes in carrier characteristics"@en ;
    rdfs:subPropertyOf <http://rdaregistry.info/Elements/m/P30214> ;
    skos:definition "Met une manifestation en relation avec une note portant sur les changements dans les caractéristiques du support matériel survenant dans les livraisons ou parties ultérieures d’une ressource publiée en parties successives ou bien entre les différentes itérations d’une ressource intégratrice."@fr, "Relates a manifestation to a note on changes in the characteristics of the carrier that occur in subsequent issues or parts of a manifestation issued in successive parts or between iterations of an integrating resource."@en .

<http://rdaregistry.info/Elements/m/P30052>
    rdakit:instructionNumber "2.17.8" ;
    rdakit:toolkitDefinition "A note providing details on place of distribution, distributor, or date of distribution, or information on changes in a place of distribution, distributor, or distributor's name."@en, "Note fournissant des précisions sur le lieu de diffusion ou de distribution, le diffuseur ou le distributeur ou sur la date de diffusion ou de distribution ou bien de l’information sur les changements de lieu de diffusion ou de distribution, ou de diffuseur ou distributeur ou de nom de diffuseur ou distributeur."@fr, "Una nota que proporciona detalles del lugar de distribución, distribuidor o fecha de distribución, o información sobre cambios en el lugar de distribución, distribuidor o nombre del distribuidor."@es ;
    rdakit:toolkitLabel "anmärkning om distributionsuppgift"@sv, "nota sobre la mención de distribución"@es, "note on distribution statement"@en, "note relative à la mention de diffusion ou de distribution"@fr ;
    reg:hasUnconstrained <http://rdaregistry.info/Elements/u/P60125> ;
    reg:lexicalAlias <http://rdaregistry.info/Elements/m/noteOnDistributionStatement.en> ;
    reg:name "noteOnDistributionStatement"@en ;
    reg:status <http://metadataregistry.org/uri/RegStatus/1001> ;
    a rdf:Property ;
    rdfs:domain <http://rdaregistry.info/Elements/c/C10007> ;
    rdfs:isDefinedBy <http://rdaregistry.info/Elements/m/> ;
    rdfs:label "a pour note relative à la mention de diffusion ou de distribution"@fr, "har anmärkning om distributionsuppgift"@sv, "has note on distribution statement"@en ;
    rdfs:subPropertyOf <http://rdaregistry.info/Elements/m/P30137> ;
    skos:definition "Met une manifestation en relation avec une note fournissant des précisions sur le lieu de diffusion ou de distribution, le diffuseur ou le distributeur ou sur la date de diffusion ou de distribution ou bien de l’information sur les changements de lieu de diffusion ou de distribution, ou de diffuseur ou distributeur ou de nom de diffuseur ou distributeur."@fr, "Relates a manifestation to a note providing details on place of distribution, distributor, or date of distribution, or information on changes in a place of distribution, distributor, or distributor's name."@en .

<http://rdaregistry.info/Elements/m/P30053>
    rdakit:instructionNumber "2.17.9" ;
    rdakit:toolkitDefinition "A note providing details on place of manufacture, manufacturer, or date of manufacture, or information on changes in a place of manufacture, manufacturer, or manufacturer's name."@en, "Note fournissant des précisions sur le lieu de fabrication, le fabricant ou la date de fabrication ou bien de l’information sur les changements de lieu de fabrication, de fabricant ou de nom de fabricant."@fr, "Una nota que proporciona detalles del lugar de fabricación, fabricantes o fecha de fabricación, o información sobre cambios en el lugar de fabricación, fabricante o fecha fabricación."@es ;
    rdakit:toolkitLabel "anmärkning om tillverkningsuppgift"@sv, "nota sobre la mención de fabricación"@es, "note on manufacture statement"@en, "note relative à la mention de fabrication"@fr ;
    reg:hasUnconstrained <http://rdaregistry.info/Elements/u/P60126> ;
    reg:lexicalAlias <http://rdaregistry.info/Elements/m/noteOnManufactureStatement.en> ;
    reg:name "noteOnManufactureStatement"@en ;
    reg:status <http://metadataregistry.org/uri/RegStatus/1001> ;
    a rdf:Property ;
    rdfs:domain <http://rdaregistry.info/Elements/c/C10007> ;
    rdfs:isDefinedBy <http://rdaregistry.info/Elements/m/> ;
    rdfs:label "a pour note relative à la mention de fabrication"@fr, "har anmärkning om tillverkningsuppgift"@sv, "has note on manufacture statement"@en ;
    rdfs:subPropertyOf <http://rdaregistry.info/Elements/m/P30137> ;
    skos:definition "Met une manifestation en relation avec une note fournissant des précisions sur le lieu de fabrication, le fabricant ou la date de fabrication ou bien de l’information sur les changements de lieu de fabrication, de fabricant ou de nom de fabricant."@fr, "Relates a manifestation to a note providing details on place of manufacture, manufacturer, or date of manufacture, or information on changes in a place of manufacture, manufacturer, or manufacturer's name."@en .

<http://rdaregistry.info/Elements/m/P30054>
    rdakit:instructionNumber "2.17.6" ;
    rdakit:toolkitDefinition "A note providing details on place of production, producer, or date of production, or information on changes in a place of production, producer, or producer's name."@en, "Note fournissant des précisions sur le lieu de production, le producteur ou la date de production ou bien de l’information sur les changements de lieu de production, de producteur ou de nom de producteur."@fr, "Una nota que proporciona detalles del lugar de producción, el productor, o la fecha producción, o información sobre cambios en el lugar de producción, el productor o el nombre del productor."@es ;
    rdakit:toolkitLabel "anmärkning om produktionsuppgift"@sv, "nota sobre la mención de producción"@es, "note on production statement"@en, "note relative à la mention de production"@fr ;
    reg:hasUnconstrained <http://rdaregistry.info/Elements/u/P60127> ;
    reg:lexicalAlias <http://rdaregistry.info/Elements/m/noteOnProductionStatement.en> ;
    reg:name "noteOnProductionStatement"@en ;
    reg:status <http://metadataregistry.org/uri/RegStatus/1001> ;
    a rdf:Property ;
    rdfs:domain <http://rdaregistry.info/Elements/c/C10007> ;
    rdfs:isDefinedBy <http://rdaregistry.info/Elements/m/> ;
    rdfs:label "a pour note relative à la mention de production"@fr, "har anmärkning om produktionsuppgift"@sv, "has note on production statement"@en ;
    rdfs:subPropertyOf <http://rdaregistry.info/Elements/m/P30137> ;
    skos:definition "Met une manifestation en relation avec une note fournissant des précisions sur le lieu de production, le producteur ou la date de production ou bien de l’information sur les changements de lieu de production, de producteur ou de nom de producteur."@fr, "Relates a manifestation to a note providing details on place of production, producer, or date of production, or information on changes in a place of production, producer, or producer's name."@en .

<http://rdaregistry.info/Elements/m/P30055>
    rdakit:instructionNumber "2.17.7" ;
    rdakit:toolkitDefinition "A note providing details on place of publication, publisher, or date of publication, or information on changes in a place of publication, publisher, or publisher's name."@en, "Note fournissant des précisions sur le lieu de publication, l’éditeur ou la date de publication ou bien de l’information sur les changements de lieu de publication, d’éditeur, ou de nom d’éditeur ou sur les interruptions de publication."@fr, "Una nota que proporciona detalles del lugar de publicación, editor o fecha de publicación, o información sobre cambios en el lugar de publicación, editor o nombre del editor."@es ;
    rdakit:toolkitLabel "anmärkning om utgivningsuppgift"@sv, "nota sobre la mención de publicación"@es, "note on publication statement"@en, "note relative à la mention de publication"@fr ;
    reg:hasUnconstrained <http://rdaregistry.info/Elements/u/P60128> ;
    reg:lexicalAlias <http://rdaregistry.info/Elements/m/noteOnPublicationStatement.en> ;
    reg:name "noteOnPublicationStatement"@en ;
    reg:status <http://metadataregistry.org/uri/RegStatus/1001> ;
    a rdf:Property ;
    rdfs:domain <http://rdaregistry.info/Elements/c/C10007> ;
    rdfs:isDefinedBy <http://rdaregistry.info/Elements/m/> ;
    rdfs:label "a pour note relative à la mention de publication"@fr, "har anmärkning om utgivningsuppgift"@sv, "has note on publication statement"@en ;
    rdfs:subPropertyOf <http://rdaregistry.info/Elements/m/P30137> ;
    skos:definition "Met une manifestation en relation avec une note fournissant des précisions sur le lieu de publication, l’éditeur ou la date de publication ou bien de l’information sur les changements de lieu de publication, d’éditeur, ou de nom d’éditeur ou sur les interruptions de publication."@fr, "Relates a manifestation to a note providing details on place of publication, publisher, or date of publication, information on changes in a place of publication, publisher, or publisher's name, or on suspension of publication."@en .

<http://rdaregistry.info/Elements/m/P30056>
    rdakit:instructionNumber "2.17.12" ;
    rdakit:toolkitDefinition "A note providing details on the currency of the contents, on the frequency of release of issues or parts of a serial or the frequency of updates to an integrating resource, or on changes in frequency."@en, "Note fournissant des précisions sur la fraîcheur du contenu, la périodicité des livraisons ou des parties d’une publication en série ou bien sur la périodicité des mises à jour d’une ressource intégratrice ou sur les changements de périodicité."@fr, "Una nota que proporciona detalles sobre la frecuencia de salida de las entregas o partes de una publicación seriada, la frecuencia de actualizaciones de un recurso integrable, la actualidad de los contenidos, o cambios en la frecuencia."@es ;
    rdakit:toolkitLabel "anmärkning om frekvens"@sv, "nota sobre la frecuencia"@es, "note on frequency"@en, "note relative à la périodicité"@fr ;
    reg:hasUnconstrained <http://rdaregistry.info/Elements/u/P60129> ;
    reg:lexicalAlias <http://rdaregistry.info/Elements/m/noteOnFrequency.en> ;
    reg:name "noteOnFrequency"@en ;
    reg:status <http://metadataregistry.org/uri/RegStatus/1001> ;
    a rdf:Property ;
    rdfs:domain <http://rdaregistry.info/Elements/c/C10007> ;
    rdfs:isDefinedBy <http://rdaregistry.info/Elements/m/> ;
    rdfs:label "a pour note relative à la périodicité"@fr, "har anmärkning om frekvens"@sv, "has note on frequency"@en ;
    rdfs:subPropertyOf <http://rdaregistry.info/Elements/m/P30137> ;
    skos:definition "Met une manifestation en relation avec une note fournissant des précisions sur la fraîcheur du contenu, la périodicité des livraisons ou des parties d’une publication en série ou bien sur la périodicité des mises à jour d’une ressource intégratrice ou sur les changements de périodicité."@fr, "Relates a manifestation to a note providing details on the currency of the contents, on the frequency of release of issues or parts of a serial or the frequency of updates to an integrating resource, or on changes in frequency."@en .

<http://rdaregistry.info/Elements/m/P30057>
    rdakit:instructionNumber "2.17.3" ;
    rdakit:toolkitDefinition "A note providing information on an agent not named in a statement of responsibility to whom responsibility for the creation of, or contribution to a realization of, the intellectual or artistic content of a work has been attributed, on variant forms of names appearing in the manifestation, on changes in statements of responsibility, or on other details relating to a statement of responsibility."@en, "Note fournissant de l’information sur une personne, une famille ou une collectivité qui n’est pas nommée dans une mention de responsabilité et à qui la responsabilité du contenu intellectuel ou artistique a été attribuée ou bien sur les variantes de forme de nom apparaissant sur la ressource, sur les changements de mentions de responsabilité ou bien sur d’autres particularités relatives aux mentions de responsabilité."@fr, "Una nota que proporciona información sobre una persona, familia, o entidad corporativa no mencionada en una mención de responsabilidad a la que se ha atribuido la responsabilidad por el contenido intelectual o artístico del recurso, formas variantes de los nombres que aparecen en el recurso, cambios en menciones de responsabilidad, u otros detalles relacionados con una mención de responsabilidad."@es ;
    rdakit:toolkitLabel "anmärkning om upphovsuppgift"@sv, "nota sobre la mención de responsabilidad"@es, "note on statement of responsibility"@en, "note relative à la mention de responsabilité"@fr ;
    reg:hasUnconstrained <http://rdaregistry.info/Elements/u/P60130> ;
    reg:lexicalAlias <http://rdaregistry.info/Elements/m/noteOnStatementOfResponsibility.en> ;
    reg:name "noteOnStatementOfResponsibility"@en ;
    reg:status <http://metadataregistry.org/uri/RegStatus/1001> ;
    a rdf:Property ;
    rdfs:domain <http://rdaregistry.info/Elements/c/C10007> ;
    rdfs:isDefinedBy <http://rdaregistry.info/Elements/m/> ;
    rdfs:label "a pour note relative à la mention de responsabilité"@fr, "har anmärkning om upphovsuppgift"@sv, "has note on statement of responsibility"@en ;
    rdfs:subPropertyOf <http://rdaregistry.info/Elements/m/P30137> ;
    skos:definition "Met une manifestation en relation avec une note fournissant de l’information sur une personne, une famille ou une collectivité qui n’est pas nommée dans une mention de responsabilité et à qui la responsabilité du contenu intellectuel ou artistique a été attribuée ou bien sur les variantes de forme de nom apparaissant sur la ressource, sur les changements de mentions de responsabilité ou bien sur d’autres particularités relatives aux mentions de responsabilité."@fr, "Relates a manifestation to a note providing information on an agent not named in a statement of responsibility to whom responsibility for the creation of, or contribution to a realization of, the intellectual or artistic content of a work has been attributed, on variant forms of names appearing in the manifestation, on changes in statements of responsibility, or on other details relating to a statement of responsibility."@en .

<http://rdaregistry.info/Elements/m/P30058>
    rdakit:instructionNumber "2.17.11" ;
    rdakit:toolkitDefinition "A note providing information on complex series statements, on incorrect numbering within series, on changes in series statements, or on other information relating to a series statement."@en, "Note fournissant de l’information sur des mentions de collection complexes, une numérotation erronée à l’intérieur de la collection, ou des changements dans les mentions de collection."@fr, "Una nota que proporciona información sobre menciones de serie complejas, numeración incorrecta dentro de la serie, o cambios en menciones de serie."@es ;
    rdakit:toolkitLabel "anmärkning om serieuppgift"@sv, "nota sobre la mención de serie"@es, "note on series statement"@en, "note relative à la mention de collection"@fr ;
    reg:hasUnconstrained <http://rdaregistry.info/Elements/u/P60131> ;
    reg:lexicalAlias <http://rdaregistry.info/Elements/m/noteOnSeriesStatement.en> ;
    reg:name "noteOnSeriesStatement"@en ;
    reg:status <http://metadataregistry.org/uri/RegStatus/1001> ;
    a rdf:Property ;
    rdfs:domain <http://rdaregistry.info/Elements/c/C10007> ;
    rdfs:isDefinedBy <http://rdaregistry.info/Elements/m/> ;
    rdfs:label "a pour note relative à la mention de collection"@fr, "har anmärkning om serieuppgift"@sv, "has note on series statement"@en ;
    rdfs:subPropertyOf <http://rdaregistry.info/Elements/m/P30137> ;
    skos:definition "Met une manifestation en relation avec une note fournissant de l’information sur des mentions de collection complexes, une numérotation erronée à l’intérieur de la collection, ou des changements dans les mentions de collection."@fr, "Relates a manifestation to a note providing information on complex series statements, on incorrect numbering within series, on changes in series statements, or on other information relating to a series statement."@en .

<http://rdaregistry.info/Elements/m/P30059>
    rdakit:instructionNumber "2.17.10" ;
    rdakit:toolkitDefinition "A note providing information on copyright dates not recorded as part of a copyright date element."@en, "Note fournissant un complément d’information sur les dates de copyright s’appliquant à divers aspects de la ressource."@fr, "Una nota que proporciona información sobre las fechas de derechos de autor como parte del elemento fecha de derechos de autor."@es ;
    rdakit:toolkitLabel "anmärkning om copyrightår"@sv, "nota sobre la fecha de copyright"@es, "note on copyright date"@en, "note relative à la date de copyright"@fr ;
    reg:hasUnconstrained <http://rdaregistry.info/Elements/u/P60132> ;
    reg:lexicalAlias <http://rdaregistry.info/Elements/m/noteOnCopyrightDate.en> ;
    reg:name "noteOnCopyrightDate"@en ;
    reg:status <http://metadataregistry.org/uri/RegStatus/1001> ;
    a rdf:Property ;
    rdfs:domain <http://rdaregistry.info/Elements/c/C10007> ;
    rdfs:isDefinedBy <http://rdaregistry.info/Elements/m/> ;
    rdfs:label "a pour note relative à la date de copyright"@fr, "har anmärkning om copyrightår"@sv, "has note on copyright date"@en ;
    rdfs:subPropertyOf <http://rdaregistry.info/Elements/m/P30137> ;
    skos:definition "Met une manifestation en relation avec une note fournissant un complément d’information sur les dates de copyright s’appliquant à divers aspects de la ressource."@fr, "Relates a manifestation to a note providing information on copyright dates not recorded as part of a copyright date element."@en .

<http://rdaregistry.info/Elements/m/P30060>
    rdakit:instructionNumber "3.21.3" ;
    rdakit:toolkitDefinition "A note providing information on the dimensions of a manifestation that is not recorded as part of a dimensions element."@en, "Note fournissant de l’information sur les dimensions d’une manifestation qui n’est pas enregistrée dans l’élément Dimensions."@fr, "Una nota que proporciona información sobre las dimensiones de la manifestación que no están registradas formalmente como parte del elemento dimensiones."@es ;
    rdakit:toolkitLabel "anmärkning om manifestationens mått"@sv, "nota sobre las dimensiones de la manifestación"@es, "note on dimensions of manifestation"@en, "note sur les dimensions de la manifestation"@fr ;
    reg:hasUnconstrained <http://rdaregistry.info/Elements/u/P60133> ;
    reg:lexicalAlias <http://rdaregistry.info/Elements/m/noteOnDimensionsOfManifestation.en> ;
    reg:name "noteOnDimensionsOfManifestation"@en ;
    reg:status <http://metadataregistry.org/uri/RegStatus/1001> ;
    a rdf:Property ;
    rdfs:domain <http://rdaregistry.info/Elements/c/C10007> ;
    rdfs:isDefinedBy <http://rdaregistry.info/Elements/m/> ;
    rdfs:label "a pour note sur les dimensions de la manifestation"@fr, "har anmärkning om manifestationens mått"@sv, "has note on dimensions of manifestation"@en ;
    rdfs:subPropertyOf <http://rdaregistry.info/Elements/m/P30214> ;
    skos:definition "Met une manifestation en relation avec une note fournissant de l’information sur les dimensions d’une manifestation qui n’est pas enregistrée dans l’élément Dimensions."@fr, "Relates a manifestation to a note providing information on the dimensions of a manifestation that is not recorded as part of a dimensions element."@en .

<http://rdaregistry.info/Elements/m/P30061>
    rdakit:instructionNumber "3.21.2" ;
    rdakit:toolkitDefinition "A note providing information on the extent of a manifestation that is not recorded as part of an extent element."@en, "Note fournissant de l’information sur l’importance matérielle de la manifestation qui n’est pas enregistrée dans l’élément Importance matérielle."@fr, "Una nota que proporciona información sobre la extensión de una manifestación que no está registrada como parte del elemento extensión."@es ;
    rdakit:toolkitLabel "anmärkning om manifestationens omfång"@sv, "nota sobre la extensión de la manifestación"@es, "note on extent of manifestation"@en, "note sur l’importance matérielle de la manifestation"@fr ;
    reg:hasUnconstrained <http://rdaregistry.info/Elements/u/P60134> ;
    reg:lexicalAlias <http://rdaregistry.info/Elements/m/noteOnExtentOfManifestation.en> ;
    reg:name "noteOnExtentOfManifestation"@en ;
    reg:status <http://metadataregistry.org/uri/RegStatus/1001> ;
    a rdf:Property ;
    rdfs:domain <http://rdaregistry.info/Elements/c/C10007> ;
    rdfs:isDefinedBy <http://rdaregistry.info/Elements/m/> ;
    rdfs:label "a pour note sur l’importance matérielle de la manifestation"@fr, "har anmärkning om manifestationens omfång"@sv, "has note on extent of manifestation"@en ;
    rdfs:subPropertyOf <http://rdaregistry.info/Elements/m/P30214> ;
    skos:definition "Met une manifestation en relation avec une note fournissant de l’information sur l’importance matérielle de la manifestation qui n’est pas enregistrée dans l’élément Importance matérielle."@fr, "Relates a manifestation to a note providing information on the extent of a manifestation that is not recorded as part of an extent element."@en .

<http://rdaregistry.info/Elements/m/P30062>
    rdakit:instructionNumber "2.17.5" ;
    rdakit:toolkitDefinition "A note providing information on the numbering of the first and/or last issue or part, on complex or irregular numbering including numbering errors, on the period covered by a volume, issue, part, etc., or on other information relating to numbering of serials."@en, "Note fournissant de l’information sur la numérotation de la première et/ou de la dernière livraison ou partie, sur une numérotation complexe ou irrégulière (y compris les erreurs de numérotation) ou sur la période couverte par un volume, une livraison, une partie, etc."@fr, "Una nota que proporciona información sobre la numeración de la primera y/o última entrega o parte, numeración compleja o irregular (incluyendo errores de numeración), o el período cubierto por un volumen, entrega o parte, etc."@es ;
    rdakit:toolkitLabel "anmärkning om numrering av seriella resurser"@sv, "nota sobre numeración de las publicaciones seriadas"@es, "note on numbering of serials"@en, "note relative à la numérotation des publications en série"@fr ;
    reg:hasUnconstrained <http://rdaregistry.info/Elements/u/P60135> ;
    reg:lexicalAlias <http://rdaregistry.info/Elements/m/noteOnNumberingOfSerials.en> ;
    reg:name "noteOnNumberingOfSerials"@en ;
    reg:status <http://metadataregistry.org/uri/RegStatus/1001> ;
    a rdf:Property ;
    rdfs:domain <http://rdaregistry.info/Elements/c/C10007> ;
    rdfs:isDefinedBy <http://rdaregistry.info/Elements/m/> ;
    rdfs:label "a pour note relative à la numérotation des publications en série"@fr, "har anmärkning om numrering av seriella resurser"@sv, "has note on numbering of serials"@en ;
    rdfs:subPropertyOf <http://rdaregistry.info/Elements/m/P30137> ;
    skos:definition "Met une manifestation en relation avec une note fournissant de l’information sur la numérotation de la première et/ou de la dernière livraison ou partie, sur une numérotation complexe ou irrégulière (y compris les erreurs de numérotation) ou sur la période couverte par un volume, une livraison, une partie, etc."@fr, "Relates a manifestation to a note providing information on the numbering of the first and/or last issue or part, on complex or irregular numbering including numbering errors, on the period covered by a volume, issue, part, etc., or on other information relating to numbering of serials."@en .

<http://rdaregistry.info/Elements/m/P30063>
    rdakit:instructionNumber "2.17.2" ;
    rdakit:toolkitDefinition "A note providing information on the source from which a title was taken, on the date the title was viewed, on variations in titles, on inaccuracies, deletions, etc., or on other information relating to a title."@en, "Note fournissant de l’information sur la source d’où est tiré un titre, la date à laquelle le titre a été vu, les variations dans les titres, les inexactitudes, les suppressions, etc. ou toute autre information relative au titre."@fr, "Una nota que proporciona información sobre la fecha en que el título fue revisado, variaciones en los títulos, inexactitudes, supresiones, etc., u otra información relacionada con el título."@es ;
    rdakit:toolkitLabel "anmärkning om titel"@sv, "nota sobre el título"@es, "note on title"@en, "note relative au titre"@fr ;
    reg:hasUnconstrained <http://rdaregistry.info/Elements/u/P60136> ;
    reg:lexicalAlias <http://rdaregistry.info/Elements/m/noteOnTitle.en> ;
    reg:name "noteOnTitle"@en ;
    reg:status <http://metadataregistry.org/uri/RegStatus/1001> ;
    a rdf:Property ;
    rdfs:domain <http://rdaregistry.info/Elements/c/C10007> ;
    rdfs:isDefinedBy <http://rdaregistry.info/Elements/m/> ;
    rdfs:label "a pour note relative au titre"@fr, "har anmärkning om titel"@sv, "has note on title"@en ;
    rdfs:subPropertyOf <http://rdaregistry.info/Elements/m/P30137> ;
    skos:definition "Met une manifestation en relation avec une note fournissant de l’information sur la source d’où est tiré un titre, la date à laquelle le titre a été vu, les variations dans les titres, les inexactitudes, les suppressions, etc. ou toute autre information relative au titre."@fr, "Relates a manifestation to a note providing information on the source from which a title was taken, on the date the title was viewed, on variations in titles, on inaccuracies, deletions, etc., or on other information relating to a title."@en .

<http://rdaregistry.info/Elements/m/P30064>
    rdakit:instructionNumber "2.17.4" ;
    rdakit:toolkitDefinition "A note providing information on the source of an edition statement, on edition statements relating to issues, parts, etc., on changes in edition statements, or on other information relating to an edition statement."@en, "Note fournissant de l’information sur la source d’une mention d’édition, sur les mentions d’édition relatives aux livraisons, parties, etc. sur les changements dans les mentions d’édition ou bien toute autre information relative à une mention d’édition."@fr, "Una nota que proporciona información sobre la fuente de una mención de edición, mención de edición relacionada con entregas, partes, etc., cambios en las menciones de edición, u otra información relacionada con una mención de edición."@es ;
    rdakit:toolkitLabel "anmärkning om upplageuppgift"@sv, "nota sobre la mención de edición"@es, "note on edition statement"@en, "note relative à la mention d’édition"@fr ;
    reg:hasUnconstrained <http://rdaregistry.info/Elements/u/P60137> ;
    reg:lexicalAlias <http://rdaregistry.info/Elements/m/noteOnEditionStatement.en> ;
    reg:name "noteOnEditionStatement"@en ;
    reg:status <http://metadataregistry.org/uri/RegStatus/1001> ;
    a rdf:Property ;
    rdfs:domain <http://rdaregistry.info/Elements/c/C10007> ;
    rdfs:isDefinedBy <http://rdaregistry.info/Elements/m/> ;
    rdfs:label "a pour note relative à la mention d’édition"@fr, "har anmärkning om upplageuppgift"@sv, "has note on edition statement"@en ;
    rdfs:subPropertyOf <http://rdaregistry.info/Elements/m/P30137> ;
    skos:definition "Met une manifestation en relation avec une note fournissant de l’information sur la source d’une mention d’édition, sur les mentions d’édition relatives aux livraisons, parties, etc. sur les changements dans les mentions d’édition ou bien toute autre information relative à une mention d’édition."@fr, "Relates a manifestation to a note providing information on the source of an edition statement, on edition statements relating to issues, parts, etc., on changes in edition statements, or on other information relating to an edition statement."@en .

<http://rdaregistry.info/Elements/m/P30065>
    rdakit:instructionNumber "2.15.2" ;
    rdakit:toolkitDefinition "A numbering designation assigned to a notated music manifestation by a publisher."@en, "Numérotation attribuée à une ressource par un éditeur de musique et qui figure normalement uniquement sur la page de titre, la couverture et/ou la première page de musique."@fr, "Una designación numérica asignada a un recurso por un editor musical. Este número aparece normalmente en la portada, la carátula y/o primera página de la música."@es ;
    rdakit:toolkitLabel "editionsnummer"@sv, "numéro d’éditeur pour la musique"@fr, "número del editor para música"@es, "publisher's number for notated music"@en ;
    reg:hasUnconstrained <http://rdaregistry.info/Elements/u/P60139> ;
    reg:lexicalAlias <http://rdaregistry.info/Elements/m/publishersNumberForNotatedMusic.en> ;
    reg:name "publishersNumberForNotatedMusic"@en ;
    reg:status <http://metadataregistry.org/uri/RegStatus/1001> ;
    a rdf:Property ;
    rdfs:domain <http://rdaregistry.info/Elements/c/C10007> ;
    rdfs:isDefinedBy <http://rdaregistry.info/Elements/m/> ;
    rdfs:label "a pour numéro d’éditeur pour la musique"@fr, "har editionsnummer"@sv, "has publisher's number for notated music"@en ;
    rdfs:subPropertyOf <http://rdaregistry.info/Elements/m/P30004> ;
    skos:definition "Met une manifestation en relation avec une numérotation attribuée à une ressource par un éditeur de musique et qui figure normalement uniquement sur la page de titre, la couverture et/ou la première page de musique."@fr, "Relates a manifestation to a numbering designation assigned to a notated music manifestation by a publisher."@en ;
    skos:scopeNote "A publisher's number for notated music sometimes includes initials, abbreviations, or words identifying the publisher."@en .

<http://rdaregistry.info/Elements/m/P30066>
    rdakit:instructionNumber "2.15.3" ;
    rdakit:toolkitDefinition "A numbering designation assigned to a notated music manifestation by a publisher."@en, "Numérotation attribuée à une ressource par un éditeur de musique."@fr, "Una designación de la numeración asignada a un recurso por un editor musical."@es ;
    rdakit:toolkitLabel "cotage pour la musique"@fr, "número de plancha para música"@es, "plate number for notated music"@en, "plåtnummer"@sv ;
    reg:hasUnconstrained <http://rdaregistry.info/Elements/u/P60140> ;
    reg:lexicalAlias <http://rdaregistry.info/Elements/m/plateNumberForNotatedMusic.en> ;
    reg:name "plateNumberForNotatedMusic"@en ;
    reg:status <http://metadataregistry.org/uri/RegStatus/1001> ;
    a rdf:Property ;
    rdfs:domain <http://rdaregistry.info/Elements/c/C10007> ;
    rdfs:isDefinedBy <http://rdaregistry.info/Elements/m/> ;
    rdfs:label "a pour cotage pour la musique"@fr, "har plåtnummer"@sv, "has plate number for notated music"@en ;
    rdfs:subPropertyOf <http://rdaregistry.info/Elements/m/P30004> ;
    skos:definition "Met une manifestation en relation avec une numérotation attribuée à une ressource par un éditeur de musique."@fr, "Relates a manifestation to a numbering designation assigned to a notated music manifestation by a publisher."@en ;
    skos:scopeNote "A plate number for notated music sometimes includes initials, abbreviations, or words identifying the publisher. It is sometimes followed by a number corresponding to the number of pages or plates or a number corresponding to an individual page or plate."@en, "La numérotation est habituellement imprimée au bas de chaque page et figure aussi parfois sur la page de titre."@fr .

<http://rdaregistry.info/Elements/m/P30067>
    rdakit:instructionNumber "18.5" ;
    rdakit:toolkitDefinition "An agent involved in broadcasting a manifestation to an audience via radio, television, webcast, etc."@en, "Personne, famille ou collectivité prenant part à la diffusion d’une manifestation à un public par la radio, la télévision, la webdiffusion, etc."@fr, "Una persona, familia o entidad corporativa involucrada en la emisión de una manifestación para una audiencia mediante la radio, televisión, transmisión virtual, etc."@es ;
    rdakit:toolkitLabel "broadcaster"@en, "diffuseur"@fr, "radiodifusor"@es ;
    reg:hasSubproperty <http://rdaregistry.info/Elements/m/object/P30067> ;
    reg:hasUnconstrained <http://rdaregistry.info/Elements/u/P60407> ;
    reg:lexicalAlias <http://rdaregistry.info/Elements/m/broadcaster.en> ;
    reg:name "broadcaster"@en ;
    reg:status <http://metadataregistry.org/uri/RegStatus/1001> ;
    a rdf:Property ;
    rdfs:domain <http://rdaregistry.info/Elements/c/C10007> ;
    rdfs:isDefinedBy <http://rdaregistry.info/Elements/m/> ;
    rdfs:label "a pour diffuseur"@fr, "has broadcaster"@en ;
    rdfs:subPropertyOf <http://rdaregistry.info/Elements/m/P30083> ;
    skos:definition "Met une manifestation en relation avec une personne, famille ou collectivité prenant part à la diffusion d’une manifestation à un public par la radio, la télévision, la webdiffusion, etc."@fr, "Relates a manifestation to an agent involved in broadcasting a manifestation to an audience via radio, television, webcast, etc."@en .

<http://rdaregistry.info/Elements/m/P30068>
    rdakit:instructionNumber "18.5" ;
    rdakit:toolkitDefinition "An agent involved in distributing a moving image manifestation to theatres or other distribution channels."@en, "Personne, famille ou collectivité prenant part à la distribution d’une manifestation d’images animées aux salles de cinéma ou aux autres réseaux de distribution."@fr, "Una persona, familia o entidad corporativa que interviene en la distribución de una manifestación de imagen en movimiento para salas de cine y otros canales de distribución."@es ;
    rdakit:toolkitLabel "distributeur de films"@fr, "distributor cinematográfico"@es, "film distributor"@en ;
    reg:hasSubproperty <http://rdaregistry.info/Elements/m/object/P30068> ;
    reg:hasUnconstrained <http://rdaregistry.info/Elements/u/P60408> ;
    reg:lexicalAlias <http://rdaregistry.info/Elements/m/filmDistributor.en> ;
    reg:name "filmDistributor"@en ;
    reg:status <http://metadataregistry.org/uri/RegStatus/1001> ;
    a rdf:Property ;
    rdfs:domain <http://rdaregistry.info/Elements/c/C10007> ;
    rdfs:isDefinedBy <http://rdaregistry.info/Elements/m/> ;
    rdfs:label "a pour distributeur de films"@fr, "has film distributor"@en ;
    rdfs:subPropertyOf <http://rdaregistry.info/Elements/m/P30080> ;
    skos:definition "Met une manifestation en relation avec une personne, famille ou collectivité prenant part à la distribution d’une manifestation d’images animées aux salles de cinéma ou aux autres réseaux de distribution."@fr, "Relates a manifestation to an agent involved in distributing a moving image manifestation to theatres or other distribution channels."@en .

<http://rdaregistry.info/Elements/m/P30069>
    rdakit:instructionNumber "18.5" ;
    rdakit:toolkitDefinition "An agent involved in manufacturing a manifestation by being responsible for the entire graphic design of a book, including arrangement of type and illustration, choice of materials, and process used."@en, "Personne, famille ou collectivité prenant part à la fabrication d’une manifestation en étant responsable de toute la conception graphique d’un livre, y compris la composition typographique, l’arrangement des illustrations, le choix des matériaux et le processus utilisé."@fr, "Una persona, familia o entidad corporativa que interviene en la fabricación de una manifestación como responsable del diseño gráfico de un libro en su totalidad, incluyendo la disposición de tipografía e ilustración, selección de materiales, y proceso empleado."@es ;
    rdakit:toolkitLabel "book designer"@en, "diseñador de libros"@es, "graphiste"@fr ;
    reg:hasSubproperty <http://rdaregistry.info/Elements/m/object/P30069> ;
    reg:hasUnconstrained <http://rdaregistry.info/Elements/u/P60409> ;
    reg:lexicalAlias <http://rdaregistry.info/Elements/m/bookDesigner.en> ;
    reg:name "bookDesigner"@en ;
    reg:status <http://metadataregistry.org/uri/RegStatus/1001> ;
    a rdf:Property ;
    rdfs:domain <http://rdaregistry.info/Elements/c/C10007> ;
    rdfs:isDefinedBy <http://rdaregistry.info/Elements/m/> ;
    rdfs:label "a pour graphiste"@fr, "has book designer"@en ;
    rdfs:subPropertyOf <http://rdaregistry.info/Elements/m/P30082> ;
    skos:definition "Met une manifestation en relation avec une personne, famille ou collectivité prenant part à la fabrication d’une manifestation en étant responsable de toute la conception graphique d’un livre, y compris la composition typographique, l’arrangement des illustrations, le choix des matériaux et le processus utilisé."@fr, "Relates a manifestation to an agent involved in manufacturing a manifestation by being responsible for the entire graphic design of a book, including arrangement of type and illustration, choice of materials, and process used."@en .

<http://rdaregistry.info/Elements/m/P30070>
    rdakit:instructionNumber "18.5" ;
    rdakit:toolkitDefinition "An agent involved in manufacturing a manifestation by cutting letters, figures, etc., on a surface such as a wooden or metal plate used for printing."@en, "Personne, famille ou collectivité prenant part à la fabrication d’une manifestation en gravant des lettres, des figures, etc. sur une surface telle qu’une plaque de bois ou de métal utilisée pour l’impression."@fr, "Una persona, familia o entidad corporativa que interviene en la fabricación de una manifestación cortando letras, figuras, etc., en una superficie utilizada para impresión como puede ser la madera o planchas de metal."@es ;
    rdakit:toolkitLabel "engraver"@en, "grabador"@es, "graveur"@fr ;
    reg:hasSubproperty <http://rdaregistry.info/Elements/m/object/P30070> ;
    reg:hasUnconstrained <http://rdaregistry.info/Elements/u/P60410> ;
    reg:lexicalAlias <http://rdaregistry.info/Elements/m/engraver.en> ;
    reg:name "engraver"@en ;
    reg:status <http://metadataregistry.org/uri/RegStatus/1001> ;
    a rdf:Property ;
    rdfs:domain <http://rdaregistry.info/Elements/c/C10007> ;
    rdfs:isDefinedBy <http://rdaregistry.info/Elements/m/> ;
    rdfs:label "a pour graveur"@fr, "has engraver"@en ;
    rdfs:subPropertyOf <http://rdaregistry.info/Elements/m/P30082> ;
    skos:definition "Met une manifestation en relation avec une personne, famille ou collectivité prenant part à la fabrication d’une manifestation en gravant des lettres, des figures, etc. sur une surface telle qu’une plaque de bois ou de métal utilisée pour l’impression."@fr, "Relates a manifestation to an agent involved in manufacturing a manifestation by cutting letters, figures, etc., on a surface such as a wooden or metal plate used for printing."@en .

<http://rdaregistry.info/Elements/m/P30071>
    rdakit:instructionNumber "18.5" ;
    rdakit:toolkitDefinition "An agent involved in manufacturing a manifestation by embossing braille cells using a stylus, special embossing printer, or other device."@en, "Personne, famille ou collectivité prenant part à la fabrication d’une manifestation par l’embossage de cellules braille au moyen d’un poinçon, d’une imprimante spéciale ou d’un autre appareil."@fr, "Una persona, familia o entidad corporativa que interviene en la fabricación de una manifestación grabando celdas Braille mediante el uso de un punzón, grabador de relieve especial u otro medio."@es ;
    rdakit:toolkitLabel "braille embosser"@en, "grabador de braille"@es, "producteur braille"@fr ;
    reg:hasSubproperty <http://rdaregistry.info/Elements/m/object/P30071> ;
    reg:hasUnconstrained <http://rdaregistry.info/Elements/u/P60411> ;
    reg:lexicalAlias <http://rdaregistry.info/Elements/m/brailleEmbosser.en> ;
    reg:name "brailleEmbosser"@en ;
    reg:status <http://metadataregistry.org/uri/RegStatus/1001> ;
    a rdf:Property ;
    rdfs:domain <http://rdaregistry.info/Elements/c/C10007> ;
    rdfs:isDefinedBy <http://rdaregistry.info/Elements/m/> ;
    rdfs:label "a pour producteur braille"@fr, "has braille embosser"@en ;
    rdfs:subPropertyOf <http://rdaregistry.info/Elements/m/P30082> ;
    skos:definition "Met une manifestation en relation avec une personne, famille ou collectivité prenant part à la fabrication d’une manifestation par l’embossage de cellules braille au moyen d’un poinçon, d’une imprimante spéciale ou d’un autre appareil."@fr, "Relates a manifestation to an agent involved in manufacturing a manifestation by embossing braille cells using a stylus, special embossing printer, or other device."@en .

<http://rdaregistry.info/Elements/m/P30072>
    rdakit:instructionNumber "18.5" ;
    rdakit:toolkitDefinition "An agent involved in manufacturing a manifestation by making a relief, intaglio, or planographic printing surface."@en, "Personne, famille ou collectivité prenant part à la fabrication d’une manifestation en préparant un élément d’impression en relief, en creux ou planographique."@fr, "Una persona, familia o entidad corporativa que interviene en la fabricación de una manifestación haciendo un relieve, tallado o superficie de impresión planográfica."@es ;
    rdakit:toolkitLabel "grabador de estampas"@es, "graveur d’estampes"@fr, "printmaker"@en ;
    reg:hasSubproperty <http://rdaregistry.info/Elements/m/object/P30072> ;
    reg:hasUnconstrained <http://rdaregistry.info/Elements/u/P60412> ;
    reg:lexicalAlias <http://rdaregistry.info/Elements/m/printmaker.en> ;
    reg:name "printmaker"@en ;
    reg:status <http://metadataregistry.org/uri/RegStatus/1001> ;
    a rdf:Property ;
    rdfs:domain <http://rdaregistry.info/Elements/c/C10007> ;
    rdfs:isDefinedBy <http://rdaregistry.info/Elements/m/> ;
    rdfs:label "a pour graveur d’estampes"@fr, "has printmaker"@en ;
    rdfs:subPropertyOf <http://rdaregistry.info/Elements/m/P30082> ;
    skos:definition "Met une manifestation en relation avec une personne, famille ou collectivité prenant part à la fabrication d’une manifestation en préparant un élément d’impression en relief, en creux ou planographique."@fr, "Relates a manifestation to an agent involved in manufacturing a manifestation by making a relief, intaglio, or planographic printing surface."@en .

<http://rdaregistry.info/Elements/m/P30073>
    rdakit:instructionNumber "18.5" ;
    rdakit:toolkitDefinition "An agent involved in manufacturing a manifestation by pouring a liquid or molten substance into a mold and leaving it to solidify to take the shape of the mold."@en, "Personne, famille ou collectivité prenant part à la fabrication d’une manifestation en versant un liquide ou une substance fondue dans un moule et en laissant ce liquide ou cette substance se solidifier pour prendre la forme du moule."@fr, "Una persona, familia o entidad corporativa que interviene en la fabricación de una manifestación mediante el vaciado de un líquido o sustancia derretida en un molde que se deja solidificar hasta tomar la forma de molde."@es ;
    rdakit:toolkitLabel "caster"@en, "fondeur"@fr, "fundidor"@es ;
    reg:hasSubproperty <http://rdaregistry.info/Elements/m/object/P30073> ;
    reg:hasUnconstrained <http://rdaregistry.info/Elements/u/P60413> ;
    reg:lexicalAlias <http://rdaregistry.info/Elements/m/caster.en> ;
    reg:name "caster"@en ;
    reg:status <http://metadataregistry.org/uri/RegStatus/1001> ;
    a rdf:Property ;
    rdfs:domain <http://rdaregistry.info/Elements/c/C10007> ;
    rdfs:isDefinedBy <http://rdaregistry.info/Elements/m/> ;
    rdfs:label "a pour fondeur"@fr, "has caster"@en ;
    rdfs:subPropertyOf <http://rdaregistry.info/Elements/m/P30082> ;
    skos:definition "Met une manifestation en relation avec une personne, famille ou collectivité prenant part à la fabrication d’une manifestation en versant un liquide ou une substance fondue dans un moule et en laissant ce liquide ou cette substance se solidifier pour prendre la forme du moule."@fr, "Relates a manifestation to an agent involved in manufacturing a manifestation by pouring a liquid or molten substance into a mold and leaving it to solidify to take the shape of the mold."@en .

<http://rdaregistry.info/Elements/m/P30074>
    rdakit:instructionNumber "18.5" ;
    rdakit:toolkitDefinition "An agent involved in manufacturing a manifestation by preparing a stone or plate for lithographic printing."@en, "Personne, famille ou collectivité prenant part à la fabrication d’une manifestation en préparant une pierre ou une plaque pour l’impression lithographique, y compris un artiste graphique créant un dessin directement sur la surface à partir de laquelle l’impression sera effectuée."@fr, "Una persona, familia o entidad corporativa que interviene en la fabricación de una manifestación preparando una piedra o lámina para impresión litográfica, incluyendo al artista gráfico que crea un diseño directamente en la superficie de la cual se hace la impresión."@es ;
    rdakit:toolkitLabel "lithographe"@fr, "lithographer"@en, "litógrafo"@es ;
    reg:hasSubproperty <http://rdaregistry.info/Elements/m/object/P30074> ;
    reg:hasUnconstrained <http://rdaregistry.info/Elements/u/P60414> ;
    reg:lexicalAlias <http://rdaregistry.info/Elements/m/lithographer.en> ;
    reg:name "lithographer"@en ;
    reg:status <http://metadataregistry.org/uri/RegStatus/1001> ;
    a rdf:Property ;
    rdfs:domain <http://rdaregistry.info/Elements/c/C10007> ;
    rdfs:isDefinedBy <http://rdaregistry.info/Elements/m/> ;
    rdfs:label "a pour lithographe"@fr, "has lithographer"@en ;
    rdfs:subPropertyOf <http://rdaregistry.info/Elements/m/P30082> ;
    skos:definition "Met une manifestation en relation avec une personne, famille ou collectivité prenant part à la fabrication d’une manifestation en préparant une pierre ou une plaque pour l’impression lithographique, y compris un artiste graphique créant un dessin directement sur la surface à partir de laquelle l’impression sera effectuée."@fr, "Relates a manifestation to an agent involved in manufacturing a manifestation by preparing a stone or plate for lithographic printing."@en ;
    skos:scopeNote "A lithographer includes a graphic artist creating a design directly on the surface from which printing will be done."@en .

<http://rdaregistry.info/Elements/m/P30075>
    rdakit:instructionNumber "18.5" ;
    rdakit:toolkitDefinition "An agent involved in manufacturing a manifestation by preparing plates used in the production of printed images or text."@en, "Personne, famille ou collectivité prenant part à la fabrication d’une manifestation en préparant les planches utilisées dans la production d’images et/ou de textes imprimés."@fr, "Una persona, familia o entidad corporativa que interviene en la fabricación de una manifestación preparando planchas utilizadas en la producción de texto e imágenes impresas."@es ;
    rdakit:toolkitLabel "grabador de planchas"@es, "graveur de planches"@fr, "platemaker"@en ;
    reg:hasSubproperty <http://rdaregistry.info/Elements/m/object/P30075> ;
    reg:hasUnconstrained <http://rdaregistry.info/Elements/u/P60415> ;
    reg:lexicalAlias <http://rdaregistry.info/Elements/m/platemaker.en> ;
    reg:name "platemaker"@en ;
    reg:status <http://metadataregistry.org/uri/RegStatus/1001> ;
    a rdf:Property ;
    rdfs:domain <http://rdaregistry.info/Elements/c/C10007> ;
    rdfs:isDefinedBy <http://rdaregistry.info/Elements/m/> ;
    rdfs:label "a pour graveur de planches"@fr, "has platemaker"@en ;
    rdfs:subPropertyOf <http://rdaregistry.info/Elements/m/P30082> ;
    skos:definition "Met une manifestation en relation avec une personne, famille ou collectivité prenant part à la fabrication d’une manifestation en préparant les planches utilisées dans la production d’images et/ou de textes imprimés."@fr, "Relates a manifestation to an agent involved in manufacturing a manifestation by preparing plates used in the production of printed images or text."@en .

<http://rdaregistry.info/Elements/m/P30076>
    rdakit:instructionNumber "18.5" ;
    rdakit:toolkitDefinition "An agent involved in manufacturing a manifestation by subjecting metal, glass, or some other surface used for printing, to acid or another corrosive substance."@en, "Personne, famille ou collectivité prenant part à la fabrication d’une manifestation en soumettant à l’acide ou à une autre substance corrosive du métal, du verre ou une autre surface utilisée pour l’impression."@fr, "Una persona, familia o entidad corporativa que interviene en la fabricación de una manifestación sometiendo metal, vidrio o alguna otra superficie utilizada para impresión, al contacto con ácido u otra substancia corrosiva."@es ;
    rdakit:toolkitLabel "aguafuertista"@es, "aquafortiste"@fr, "etcher"@en ;
    reg:hasSubproperty <http://rdaregistry.info/Elements/m/object/P30076> ;
    reg:hasUnconstrained <http://rdaregistry.info/Elements/u/P60416> ;
    reg:lexicalAlias <http://rdaregistry.info/Elements/m/etcher.en> ;
    reg:name "etcher"@en ;
    reg:status <http://metadataregistry.org/uri/RegStatus/1001> ;
    a rdf:Property ;
    rdfs:domain <http://rdaregistry.info/Elements/c/C10007> ;
    rdfs:isDefinedBy <http://rdaregistry.info/Elements/m/> ;
    rdfs:label "a pour aquafortiste"@fr, "has etcher"@en ;
    rdfs:subPropertyOf <http://rdaregistry.info/Elements/m/P30082> ;
    skos:definition "Met une manifestation en relation avec une personne, famille ou collectivité prenant part à la fabrication d’une manifestation en soumettant à l’acide ou à une autre substance corrosive du métal, du verre ou une autre surface utilisée pour l’impression."@fr, "Relates a manifestation to an agent involved in manufacturing a manifestation by subjecting metal, glass, or some other surface used for printing, to acid or another corrosive substance."@en .

<http://rdaregistry.info/Elements/m/P30077>
    rdakit:instructionNumber "18.5" ;
    rdakit:toolkitDefinition "An agent involved in manufacturing a manifestation by using a photomechanical process for making prints directly from a hardened film of gelatin or other colloid that has ink-receptive and ink-repellent surfaces."@en, "Personne, famille ou collectivité prenant part à la fabrication d’une manifestation d’épreuves photographiques faites à partir d’un film de gélatine ou d’un autre colloïde ayant des surfaces acceptant ou repoussant l’encre."@fr, "Una persona, familia o entidad corporativa que interviene en la fabricación de una manifestación compuesta de impresiones fotográficas sobre película u otro coloide con superficies receptivas y repelentes a la tinta."@es ;
    rdakit:toolkitLabel "collotyper"@en, "fototipista"@es, "phototypeur"@fr ;
    reg:hasSubproperty <http://rdaregistry.info/Elements/m/object/P30077> ;
    reg:hasUnconstrained <http://rdaregistry.info/Elements/u/P60417> ;
    reg:lexicalAlias <http://rdaregistry.info/Elements/m/collotyper.en> ;
    reg:name "collotyper"@en ;
    reg:status <http://metadataregistry.org/uri/RegStatus/1001> ;
    a rdf:Property ;
    rdfs:domain <http://rdaregistry.info/Elements/c/C10007> ;
    rdfs:isDefinedBy <http://rdaregistry.info/Elements/m/> ;
    rdfs:label "a pour phototypeur"@fr, "has collotyper"@en ;
    rdfs:subPropertyOf <http://rdaregistry.info/Elements/m/P30082> ;
    skos:definition "Met une manifestation en relation avec une personne, famille ou collectivité prenant part à la fabrication d’une manifestation d’épreuves photographiques faites à partir d’un film de gélatine ou d’un autre colloïde ayant des surfaces acceptant ou repoussant l’encre."@fr, "Relates a manifestation to an agent involved in manufacturing a manifestation by using a photomechanical process for making prints directly from a hardened film of gelatin or other colloid that has ink-receptive and ink-repellent surfaces."@en .

<http://rdaregistry.info/Elements/m/P30078>
    rdakit:instructionNumber "18.5" ;
    rdakit:toolkitDefinition "An agent involved in manufacturing a manifestation of printed text, notated music, etc., from type or plates, such as a book, newspaper, magazine, broadside, score, etc."@en, "Personne, famille ou collectivité prenant part à la fabrication d’une manifestation de texte imprimé, de musique notée, etc. à partir de caractères ou de planches, telle qu’un livre, un journal, une revue, un placard, une partition, etc."@fr, "Una persona, familia o entidad corporativa que interviene en la fabricación de una manifestación de texto impreso, música notada, etc., tal como un libro, periódico, revista, pliego suelto, partitura, etc., mediante tipos o planchas."@es ;
    rdakit:toolkitLabel "impresor"@es, "imprimeur"@fr, "printer"@en ;
    reg:hasSubproperty <http://rdaregistry.info/Elements/m/object/P30078> ;
    reg:hasUnconstrained <http://rdaregistry.info/Elements/u/P60418> ;
    reg:lexicalAlias <http://rdaregistry.info/Elements/m/printer.en> ;
    reg:name "printer"@en ;
    reg:status <http://metadataregistry.org/uri/RegStatus/1001> ;
    a rdf:Property ;
    rdfs:domain <http://rdaregistry.info/Elements/c/C10007> ;
    rdfs:isDefinedBy <http://rdaregistry.info/Elements/m/> ;
    rdfs:label "a pour imprimeur"@fr, "has printer"@en ;
    rdfs:subPropertyOf <http://rdaregistry.info/Elements/m/P30082> ;
    skos:definition "Met une manifestation en relation avec une personne, famille ou collectivité prenant part à la fabrication d’une manifestation de texte imprimé, de musique notée, etc. à partir de caractères ou de planches, telle qu’un livre, un journal, une revue, un placard, une partition, etc."@fr, "Relates a manifestation to an agent involved in manufacturing a manifestation of printed text, notated music, etc., from type or plates, such as a book, newspaper, magazine, broadside, score, etc."@en .

<http://rdaregistry.info/Elements/m/P30079>
    rdakit:instructionNumber "21.6" ;
    rdakit:toolkitDefinition "An agent other than a producer, publisher, distributor, or manufacturer associated with a manifestation."@en, "Personne, famille ou collectivité, autre qu’un producteur, un éditeur, un diffuseur ou distributeur ou bien un fabricant, associée à une manifestation."@fr, "Una persona, familia o entidad corporativa diferente a un productor, editor, distribuidor o fabricante que está asociada con una manifestación."@es ;
    rdakit:toolkitLabel "autre personne, famille ou collectivité associée à une manifestation"@fr, "other agent associated with manifestation"@en, "otra persona, familia o entidad corporativa asociada con una manifestación"@es, "övrig person, familj/släkt eller institution knuten till en manifestation"@sv ;
    reg:hasSubproperty <http://rdaregistry.info/Elements/m/object/P30079> ;
    reg:hasUnconstrained <http://rdaregistry.info/Elements/u/P60374> ;
    reg:lexicalAlias <http://rdaregistry.info/Elements/m/otherAgentManifestation.en> ;
    reg:name "otherAgentManifestation"@en ;
    reg:status <http://metadataregistry.org/uri/RegStatus/1001> ;
    a rdf:Property ;
    rdfs:domain <http://rdaregistry.info/Elements/c/C10007> ;
    rdfs:isDefinedBy <http://rdaregistry.info/Elements/m/> ;
    rdfs:label "a pour autre personne, famille ou collectivité associée à une manifestation"@fr, "har övrig person, familj/släkt eller institution knuten till en manifestation"@sv, "has other agent associated with manifestation"@en ;
    rdfs:subPropertyOf <http://rdaregistry.info/Elements/m/P30267> ;
    skos:definition "Met une manifestation en relation avec une personne, famille ou collectivité, autre qu’un producteur, un éditeur, un diffuseur ou distributeur ou bien un fabricant, associée à une manifestation."@fr, "Relates a manifestation to an agent other than a producer, publisher, distributor, or manufacturer associated with a manifestation."@en ;
    skos:scopeNote "Book designers, platemakers, etc., are included."@en, "Comprend les graphistes, les graveurs de planches, etc."@fr .

<http://rdaregistry.info/Elements/m/P30080>
    rdakit:instructionNumber "21.4" ;
    rdakit:toolkitDefinition "An agent responsible for distributing a manifestation."@en, "Personne, famille ou collectivité responsable de la diffusion ou de la distribution d’une ressource."@fr, "Una persona, familia o entidad corporativa responsable de la distribución de un recurso."@es ;
    rdakit:toolkitLabel "diffuseur ou distributeur"@fr, "distribuidor"@es, "distributor"@en, "distributör"@sv ;
    reg:hasSubproperty <http://rdaregistry.info/Elements/m/P30068>, <http://rdaregistry.info/Elements/m/object/P30080> ;
    reg:hasUnconstrained <http://rdaregistry.info/Elements/u/P60438> ;
    reg:lexicalAlias <http://rdaregistry.info/Elements/m/distributor.en> ;
    reg:name "distributor"@en ;
    reg:status <http://metadataregistry.org/uri/RegStatus/1001> ;
    a rdf:Property ;
    rdfs:domain <http://rdaregistry.info/Elements/c/C10007> ;
    rdfs:isDefinedBy <http://rdaregistry.info/Elements/m/> ;
    rdfs:label "a pour diffuseur ou distributeur"@fr, "har distributör"@sv, "has distributor"@en ;
    rdfs:subPropertyOf <http://rdaregistry.info/Elements/m/P30267> ;
    skos:definition "Met une manifestation en relation avec une personne, famille ou collectivité responsable de la diffusion ou de la distribution d’une ressource."@fr, "Relates a manifestation to an agent responsible for distributing a manifestation."@en .

<http://rdaregistry.info/Elements/m/P30081>
    rdakit:instructionNumber "21.2" ;
    rdakit:toolkitDefinition "An agent responsible for inscribing, fabricating, constructing, etc., a manifestation in an unpublished form."@en, "Personne, famille ou collectivité responsable de la scription, de la fabrication, de la construction, etc. d’une ressource sous une forme non publiée."@fr, "Una persona, familia o entidad corporativa responsable de que se inscriba, fabrique o construya, etc., un recurso inédito."@es ;
    rdakit:toolkitLabel "producent av opublicerad resurs"@sv, "producer of unpublished manifestation"@en, "producteur d’une ressource non publiée"@fr, "productor de un recurso inédito"@es ;
    reg:hasSubproperty <http://rdaregistry.info/Elements/m/object/P30081> ;
    reg:hasUnconstrained <http://rdaregistry.info/Elements/u/P60440> ;
    reg:lexicalAlias <http://rdaregistry.info/Elements/m/producerOfUnpublishedManifestation.en> ;
    reg:name "producerOfUnpublishedManifestation"@en ;
    reg:status <http://metadataregistry.org/uri/RegStatus/1001> ;
    a rdf:Property ;
    rdfs:domain <http://rdaregistry.info/Elements/c/C10007> ;
    rdfs:isDefinedBy <http://rdaregistry.info/Elements/m/> ;
    rdfs:label "a pour producteur d’une ressource non publiée"@fr, "har producent av opublicerad resurs"@sv, "has producer of unpublished manifestation"@en ;
    rdfs:subPropertyOf <http://rdaregistry.info/Elements/m/P30267> ;
    skos:definition "Met une manifestation en relation avec une personne, famille ou collectivité responsable de la scription, de la fabrication, de la construction, etc. d’une ressource sous une forme non publiée."@fr, "Relates a manifestation to an agent responsible for inscribing, fabricating, constructing, etc., a manifestation in an unpublished form."@en .

<http://rdaregistry.info/Elements/m/P30082>
    rdakit:instructionNumber "21.5" ;
    rdakit:toolkitDefinition "An agent responsible for printing, duplicating, casting, etc., a manifestation in a published form."@en, "Personne, famille ou collectivité responsable de l’impression, de la reproduction, du moulage, etc. d’une ressource sous une forme publiée."@fr, "Una persona, familia o entidad corporativa responsable de la impresión, duplicación, prensado, etc., de un recurso publicado."@es ;
    rdakit:toolkitLabel "fabricant"@fr, "fabricante"@es, "manufacturer"@en, "tillverkare"@sv ;
    reg:hasSubproperty <http://rdaregistry.info/Elements/m/P30069>, <http://rdaregistry.info/Elements/m/P30070>, <http://rdaregistry.info/Elements/m/P30071>, <http://rdaregistry.info/Elements/m/P30072>, <http://rdaregistry.info/Elements/m/P30073>, <http://rdaregistry.info/Elements/m/P30074>, <http://rdaregistry.info/Elements/m/P30075>, <http://rdaregistry.info/Elements/m/P30076>, <http://rdaregistry.info/Elements/m/P30077>, <http://rdaregistry.info/Elements/m/P30078>, <http://rdaregistry.info/Elements/m/P30215>, <http://rdaregistry.info/Elements/m/object/P30082> ;
    reg:hasUnconstrained <http://rdaregistry.info/Elements/u/P60443> ;
    reg:lexicalAlias <http://rdaregistry.info/Elements/m/manufacturer.en> ;
    reg:name "manufacturer"@en ;
    reg:status <http://metadataregistry.org/uri/RegStatus/1001> ;
    a rdf:Property ;
    rdfs:domain <http://rdaregistry.info/Elements/c/C10007> ;
    rdfs:isDefinedBy <http://rdaregistry.info/Elements/m/> ;
    rdfs:label "a pour fabricant"@fr, "har tillverkare"@sv, "has manufacturer"@en ;
    rdfs:subPropertyOf <http://rdaregistry.info/Elements/m/P30267> ;
    skos:definition "Met une manifestation en relation avec une personne, famille ou collectivité responsable de l’impression, de la reproduction, du moulage, etc. d’une ressource sous une forme publiée."@fr, "Relates a manifestation to an agent responsible for printing, duplicating, casting, etc., a manifestation in a published form."@en .

<http://rdaregistry.info/Elements/m/P30083>
    rdakit:instructionNumber "21.3" ;
    rdakit:toolkitDefinition "An agent responsible for publishing, releasing, or issuing a manifestation."@en, "Personne, famille ou collectivité responsable de la publication, de la mise à disposition ou de l’édition d’une ressource."@fr, "Una persona, familia o entidad corporativa responsable de la publicación, lanzamiento o publicación de un recurso."@es ;
    rdakit:toolkitLabel "editor"@es, "publisher"@en, "utgivare"@sv, "éditeur"@fr ;
    reg:hasSubproperty <http://rdaregistry.info/Elements/m/P30067>, <http://rdaregistry.info/Elements/m/object/P30083> ;
    reg:hasUnconstrained <http://rdaregistry.info/Elements/u/P60444> ;
    reg:lexicalAlias <http://rdaregistry.info/Elements/m/publisher.en> ;
    reg:name "publisher"@en ;
    reg:status <http://metadataregistry.org/uri/RegStatus/1001> ;
    a rdf:Property ;
    rdfs:domain <http://rdaregistry.info/Elements/c/C10007> ;
    rdfs:isDefinedBy <http://rdaregistry.info/Elements/m/> ;
    rdfs:label "a pour éditeur"@fr, "har utgivare"@sv, "has publisher"@en ;
    rdfs:subPropertyOf <http://rdaregistry.info/Elements/m/P30267> ;
    skos:definition "Met une manifestation en relation avec une personne, famille ou collectivité responsable de la publication, de la mise à disposition ou de l’édition d’une ressource."@fr, "Relates a manifestation to an agent responsible for publishing, releasing, or issuing a manifestation."@en .

<http://rdaregistry.info/Elements/m/P30084>
    rdakit:instructionNumber "3.7" ;
    rdakit:toolkitDefinition "A physical or chemical substance applied to a base material of a manifestation."@en, "Substance physique ou chimique appliquée sur le matériau de base de la ressource."@fr, "Una sustancia física o química aplicada al material de base de un recurso."@es ;
    rdakit:toolkitLabel "applicerat material"@sv, "applied material"@en, "material aplicado"@es, "matériau appliqué"@fr ;
    reg:hasSubproperty <http://rdaregistry.info/Elements/m/P30122> ;
    reg:hasUnconstrained <http://rdaregistry.info/Elements/u/P60159> ;
    reg:lexicalAlias <http://rdaregistry.info/Elements/m/appliedMaterial.en> ;
    reg:name "appliedMaterial"@en ;
    reg:status <http://metadataregistry.org/uri/RegStatus/1001> ;
    a rdf:Property ;
    rdfs:domain <http://rdaregistry.info/Elements/c/C10007> ;
    rdfs:isDefinedBy <http://rdaregistry.info/Elements/m/> ;
    rdfs:label "a pour matériau appliqué"@fr, "har applicerat material"@sv, "has applied material"@en ;
    skos:definition "Met une manifestation en relation avec une substance physique ou chimique appliquée sur le matériau de base de la ressource."@fr, "Relates a manifestation to a physical or chemical substance applied to a base material of a manifestation."@en .

<http://rdaregistry.info/Elements/m/P30085>
    rdakit:instructionNumber "2.9.2" ;
    rdakit:toolkitDefinition "A place associated with the distribution of a manifestation in a published form."@en, "Lieu associé à la diffusion ou à la distribution d’une ressource sous une forme publiée."@fr, "Un lugar asociado con la distribución de un recurso publicado."@es ;
    rdakit:toolkitLabel "distributionsort"@sv, "lieu de diffusion ou de distribution"@fr, "lugar de distribución"@es, "place of distribution"@en ;
    reg:hasUnconstrained <http://rdaregistry.info/Elements/u/P60160> ;
    reg:lexicalAlias <http://rdaregistry.info/Elements/m/placeOfDistribution.en> ;
    reg:name "placeOfDistribution"@en ;
    reg:status <http://metadataregistry.org/uri/RegStatus/1001> ;
    a rdf:Property ;
    rdfs:domain <http://rdaregistry.info/Elements/c/C10007> ;
    rdfs:isDefinedBy <http://rdaregistry.info/Elements/m/> ;
    rdfs:label "a pour lieu de diffusion ou de distribution"@fr, "har distributionsort"@sv, "has place of distribution"@en ;
    skos:definition "Met une manifestation en relation avec un lieu associé à la diffusion ou à la distribution d’une ressource sous une forme publiée."@fr, "Relates a manifestation to a place associated with the distribution of a manifestation in a published form."@en .

<http://rdaregistry.info/Elements/m/P30086>
    rdakit:instructionNumber "2.7.2" ;
    rdakit:toolkitDefinition "A place associated with the inscription, fabrication, construction, etc., of a manifestation in an unpublished form."@en, "Lieu associé à la scription, la fabrication, la construction, etc. d’une ressource sous une forme non publiée."@fr, "Un lugar asociado con la inscripción, fabricación, construcción, etc., de un recurso en formato inédito."@es ;
    rdakit:toolkitLabel "lieu de production"@fr, "lugar de producción"@es, "place of production"@en, "produktionsort"@sv ;
    reg:hasUnconstrained <http://rdaregistry.info/Elements/u/P60161> ;
    reg:lexicalAlias <http://rdaregistry.info/Elements/m/placeOfProduction.en> ;
    reg:name "placeOfProduction"@en ;
    reg:status <http://metadataregistry.org/uri/RegStatus/1001> ;
    a rdf:Property ;
    rdfs:domain <http://rdaregistry.info/Elements/c/C10007> ;
    rdfs:isDefinedBy <http://rdaregistry.info/Elements/m/> ;
    rdfs:label "a pour lieu de production"@fr, "har produktionsort"@sv, "has place of production"@en ;
    skos:definition "Met une manifestation en relation avec un lieu associé à la scription, la fabrication, la construction, etc. d’une ressource sous une forme non publiée."@fr, "Relates a manifestation to a place associated with the inscription, fabrication, construction, etc., of a manifestation in an unpublished form."@en .

<http://rdaregistry.info/Elements/m/P30087>
    rdakit:instructionNumber "2.10.2" ;
    rdakit:toolkitDefinition "A place associated with the printing, duplicating, casting, etc., of a manifestation in a published form."@en, "Lieu associé à l’impression, à la reproduction, au moulage, etc. d’une ressource sous une forme publiée."@fr, "Un lugar asociado con la impresión, duplicación, producción, etc., de un recurso publicado."@es ;
    rdakit:toolkitLabel "lieu de fabrication"@fr, "lugar de fabricación"@es, "place of manufacture"@en, "tillverkningsort"@sv ;
    reg:hasUnconstrained <http://rdaregistry.info/Elements/u/P60162> ;
    reg:lexicalAlias <http://rdaregistry.info/Elements/m/placeOfManufacture.en> ;
    reg:name "placeOfManufacture"@en ;
    reg:status <http://metadataregistry.org/uri/RegStatus/1001> ;
    a rdf:Property ;
    rdfs:domain <http://rdaregistry.info/Elements/c/C10007> ;
    rdfs:isDefinedBy <http://rdaregistry.info/Elements/m/> ;
    rdfs:label "a pour lieu de fabrication"@fr, "har tillverkningsort"@sv, "has place of manufacture"@en ;
    skos:definition "Met une manifestation en relation avec un lieu associé à l’impression, à la reproduction, au moulage, etc. d’une ressource sous une forme publiée."@fr, "Relates a manifestation to a place associated with the printing, duplicating, casting, etc., of a manifestation in a published form."@en .

<http://rdaregistry.info/Elements/m/P30088>
    rdakit:instructionNumber "2.8.2" ;
    rdakit:toolkitDefinition "A place associated with the publication, release, or issuing of a manifestation."@en, "Lieu associé à la publication, la mise à disposition ou l’édition d’une ressource."@fr, "Un lugar asociado con la publicación, lanzamiento o edición de un recurso."@es ;
    rdakit:toolkitLabel "lieu de publication"@fr, "lugar de publicación"@es, "place of publication"@en, "utgivningsort"@sv ;
    reg:hasUnconstrained <http://rdaregistry.info/Elements/u/P60163> ;
    reg:lexicalAlias <http://rdaregistry.info/Elements/m/placeOfPublication.en> ;
    reg:name "placeOfPublication"@en ;
    reg:status <http://metadataregistry.org/uri/RegStatus/1001> ;
    a rdf:Property ;
    rdfs:domain <http://rdaregistry.info/Elements/c/C10007> ;
    rdfs:isDefinedBy <http://rdaregistry.info/Elements/m/> ;
    rdfs:label "a pour lieu de publication"@fr, "har utgivningsort"@sv, "has place of publication"@en ;
    skos:definition "Met une manifestation en relation avec un lieu associé à la publication, la mise à disposition ou l’édition d’une ressource."@fr, "Relates a manifestation to a place associated with the publication, release, or issuing of a manifestation."@en .

<http://rdaregistry.info/Elements/m/P30089>
    rdakit:instructionNumber "2.9.3" ;
    rdakit:toolkitDefinition "A place of distribution in a language or script that differs from that recorded in a place of distribution element."@en, "Lieu de diffusion ou de distribution dans une langue et/ou une écriture différentes de celles enregistrées dans l’élément Lieu de diffusion ou de distribution."@fr, "Un lugar de distribución en una lengua y/o escritura que difiere de la registrada en el elemento lugar de distribución."@es ;
    rdakit:toolkitLabel "forme parallèle du lieu de diffusion ou de distribution"@fr, "lugar paralelo de distribución"@es, "parallel place of distribution"@en, "parallell distributionsort"@sv ;
    reg:hasUnconstrained <http://rdaregistry.info/Elements/u/P60164> ;
    reg:lexicalAlias <http://rdaregistry.info/Elements/m/parallelPlaceOfDistribution.en> ;
    reg:name "parallelPlaceOfDistribution"@en ;
    reg:status <http://metadataregistry.org/uri/RegStatus/1001> ;
    a rdf:Property ;
    rdfs:domain <http://rdaregistry.info/Elements/c/C10007> ;
    rdfs:isDefinedBy <http://rdaregistry.info/Elements/m/> ;
    rdfs:label "a pour forme parallèle du lieu de diffusion ou de distribution"@fr, "har parallell distributionsort"@sv, "has parallel place of distribution"@en ;
    skos:definition "Met une manifestation en relation avec un lieu de diffusion ou de distribution dans une langue et/ou une écriture différentes de celles enregistrées dans l’élément Lieu de diffusion ou de distribution."@fr, "Relates a manifestation to a place of distribution in a language or script that differs from that recorded in a place of distribution element."@en .

<http://rdaregistry.info/Elements/m/P30090>
    rdakit:instructionNumber "2.10.3" ;
    rdakit:toolkitDefinition "A place of manufacture in a language or script that differs from that recorded in a place of manufacture element."@en, "Lieu de fabrication dans une langue et/ou une écriture différentes de celles enregistrées dans l’élément Lieu de fabrication."@fr, "Un lugar de fabricación en una lengua y/o escritura que difiere de la registrada en el elemento lugar de fabricación"@es ;
    rdakit:toolkitLabel "forme parallèle du lieu de fabrication"@fr, "lugar paralelo de fabricación"@es, "parallel place of manufacture"@en, "parallell tillverkningsort"@sv ;
    reg:hasUnconstrained <http://rdaregistry.info/Elements/u/P60165> ;
    reg:lexicalAlias <http://rdaregistry.info/Elements/m/parallelPlaceOfManufacture.en> ;
    reg:name "parallelPlaceOfManufacture"@en ;
    reg:status <http://metadataregistry.org/uri/RegStatus/1001> ;
    a rdf:Property ;
    rdfs:domain <http://rdaregistry.info/Elements/c/C10007> ;
    rdfs:isDefinedBy <http://rdaregistry.info/Elements/m/> ;
    rdfs:label "a pour forme parallèle du lieu de fabrication"@fr, "har parallell tillverkningsort"@sv, "has parallel place of manufacture"@en ;
    skos:definition "Met une manifestation en relation avec un lieu de fabrication dans une langue et/ou une écriture différentes de celles enregistrées dans l’élément Lieu de fabrication."@fr, "Relates a manifestation to a place of manufacture in a language or script that differs from that recorded in a place of manufacture element."@en .

<http://rdaregistry.info/Elements/m/P30091>
    rdakit:instructionNumber "2.7.3" ;
    rdakit:toolkitDefinition "A place of production in a language or script that differs from that recorded in a place of production element."@en, "Lieu de production dans une langue et/ou une écriture différentes de celles enregistrées dans l’élément Lieu de production."@fr, "Un lugar de producción en una lengua y/o escritura que difiere de la registrada en el elemento lugar de producción."@es ;
    rdakit:toolkitLabel "forme parallèle du lieu de production"@fr, "lugar paralelo de producción"@es, "parallel place of production"@en, "parallell produktionsort"@sv ;
    reg:hasUnconstrained <http://rdaregistry.info/Elements/u/P60166> ;
    reg:lexicalAlias <http://rdaregistry.info/Elements/m/parallelPlaceOfProduction.en> ;
    reg:name "parallelPlaceOfProduction"@en ;
    reg:status <http://metadataregistry.org/uri/RegStatus/1001> ;
    a rdf:Property ;
    rdfs:domain <http://rdaregistry.info/Elements/c/C10007> ;
    rdfs:isDefinedBy <http://rdaregistry.info/Elements/m/> ;
    rdfs:label "a pour forme parallèle du lieu de production"@fr, "har parallell produktionsort"@sv, "has parallel place of production"@en ;
    skos:definition "Met une manifestation en relation avec un lieu de production dans une langue et/ou une écriture différentes de celles enregistrées dans l’élément Lieu de production."@fr, "Relates a manifestation to a place of production in a language or script that differs from that recorded in a place of production element."@en .

<http://rdaregistry.info/Elements/m/P30092>
    rdakit:instructionNumber "2.8.3" ;
    rdakit:toolkitDefinition "A place of publication in a language or script that differs from that recorded in a place of publication element."@en, "Lieu de publication dans une langue et/ou une écriture différentes de celles enregistrées dans l’élément Lieu de publication."@fr, "Un lugar de publicación en una lengua y/o escritura que difiere de la registrada en el elemento lugar de publicación"@es ;
    rdakit:toolkitLabel "forme parallèle du lieu de publication"@fr, "lugar paralelo de publicación"@es, "parallel place of publication"@en, "parallell utgivningsort"@sv ;
    reg:hasUnconstrained <http://rdaregistry.info/Elements/u/P60167> ;
    reg:lexicalAlias <http://rdaregistry.info/Elements/m/parallelPlaceOfPublication.en> ;
    reg:name "parallelPlaceOfPublication"@en ;
    reg:status <http://metadataregistry.org/uri/RegStatus/1001> ;
    a rdf:Property ;
    rdfs:domain <http://rdaregistry.info/Elements/c/C10007> ;
    rdfs:isDefinedBy <http://rdaregistry.info/Elements/m/> ;
    rdfs:label "a pour forme parallèle du lieu de publication"@fr, "har parallell utgivningsort"@sv, "has parallel place of publication"@en ;
    skos:definition "Met une manifestation en relation avec un lieu de publication dans une langue et/ou une écriture différentes de celles enregistrées dans l’élément Lieu de publication."@fr, "Relates a manifestation to a place of publication in a language or script that differs from that recorded in a place of publication element."@en .

<http://rdaregistry.info/Elements/m/P30093>
    rdakit:instructionNumber "24.5" ;
    rdakit:toolkitDefinition "A printed manifestation that is used as the basis for a reissue of a manifestation."@en, "Manifestation imprimée servant de base à une réédition d’une manifestation."@fr, "Una manifestación impresa que es usada como base para una reedición de una manifestación."@es ;
    rdakit:toolkitLabel "reimpresión de (manifestación)"@es, "reprint of (manifestation)"@en, "réimpression de (manifestation)"@fr ;
    reg:hasSubproperty <http://rdaregistry.info/Elements/m/object/P30093> ;
    reg:hasUnconstrained <http://rdaregistry.info/Elements/u/P60168> ;
    reg:lexicalAlias <http://rdaregistry.info/Elements/m/reprintOfManifestation.en> ;
    reg:name "reprintOfManifestation"@en ;
    reg:status <http://metadataregistry.org/uri/RegStatus/1001> ;
    a rdf:Property ;
    rdfs:domain <http://rdaregistry.info/Elements/c/C10007> ;
    rdfs:isDefinedBy <http://rdaregistry.info/Elements/m/> ;
    rdfs:label "est la réimpression de (manifestation)"@fr, "is reprint of (manifestation)"@en ;
    rdfs:subPropertyOf <http://rdaregistry.info/Elements/m/P30043> ;
    skos:definition "Met une manifestation en relation avec une manifestation imprimée servant de base à une réédition d’une manifestation."@fr, "Relates a manifestation to a printed manifestation that is used as the basis for a reissue of a manifestation."@en .

<http://rdaregistry.info/Elements/m/P30094>
    rdakit:instructionNumber "2.7.5" ;
    rdakit:toolkitDefinition "A producer's name in a language or script that differs from that recorded in a producer's name element."@en, "Nom du producteur dans une langue et/ou une écriture différentes de celles enregistrées dans l’élément Nom du producteur."@fr, "Un nombre de productor en una lengua y/o escritura que difiere de la registrada en el elemento nombre del productor."@es ;
    rdakit:toolkitLabel "forme parallèle du nom du producteur"@fr, "nombre paralelo del productor"@es, "parallel producer's name"@en, "parallellt producentnamn"@sv ;
    reg:hasUnconstrained <http://rdaregistry.info/Elements/u/P60172> ;
    reg:lexicalAlias <http://rdaregistry.info/Elements/m/parallelProducersName.en> ;
    reg:name "parallelProducersName"@en ;
    reg:status <http://metadataregistry.org/uri/RegStatus/1001> ;
    a rdf:Property ;
    rdfs:domain <http://rdaregistry.info/Elements/c/C10007> ;
    rdfs:isDefinedBy <http://rdaregistry.info/Elements/m/> ;
    rdfs:label "a pour forme parallèle du nom du producteur"@fr, "har parallellt producentnamn"@sv, "has parallel producer’s name"@en ;
    skos:definition "Met une manifestation en relation avec un nom du producteur dans une langue et/ou une écriture différentes de celles enregistrées dans l’élément Nom du producteur."@fr, "Relates a manifestation to a producer's name in a language or script that differs from that recorded in a producer's name element."@en .

<http://rdaregistry.info/Elements/m/P30095>
    rdakit:instructionNumber "2.8.5" ;
    rdakit:toolkitDefinition "A publisher's name in a language or script that differs from that recorded in a publisher's name element."@en, "Nom d’éditeur dans une langue et/ou une écriture différentes de celles enregistrées dans l’élément Nom d’éditeur."@fr, "Un nombre del editor en una lengua y/o escritura que difiere de la registrada en el elemento nombre del editor."@es ;
    rdakit:toolkitLabel "forme parallèle du nom de l’éditeur"@fr, "nombre paralelo del editor"@es, "parallel publisher's name"@en, "parallellt utgivarnamn"@sv ;
    reg:hasUnconstrained <http://rdaregistry.info/Elements/u/P60173> ;
    reg:lexicalAlias <http://rdaregistry.info/Elements/m/parallelPublishersName.en> ;
    reg:name "parallelPublishersName"@en ;
    reg:status <http://metadataregistry.org/uri/RegStatus/1001> ;
    a rdf:Property ;
    rdfs:domain <http://rdaregistry.info/Elements/c/C10007> ;
    rdfs:isDefinedBy <http://rdaregistry.info/Elements/m/> ;
    rdfs:label "a pour forme parallèle du nom de l’éditeur"@fr, "har parallellt utgivarnamn"@sv, "has parallel publisher’s name"@en ;
    skos:definition "Met une manifestation en relation avec un nom d’éditeur dans une langue et/ou une écriture différentes de celles enregistrées dans l’élément Nom d’éditeur."@fr, "Relates a manifestation to a publisher's name in a language or script that differs from that recorded in a publisher's name element."@en .

<http://rdaregistry.info/Elements/m/P30096>
    rdakit:instructionNumber "3.19.3" ;
    rdakit:toolkitDefinition "A schema, standard, etc., used to encode the digital content of a manifestation."@en, "Norme, schéma, etc. utilisé pour encoder le contenu numérique d’une ressource."@fr, "Un esquema, estándar, etc., utilizado para codificar el contenido digital de un recurso."@es ;
    rdakit:toolkitLabel "encoding format"@en, "format d’encodage"@fr, "formato de codificación"@es, "kodningsformat"@sv ;
    reg:hasUnconstrained <http://rdaregistry.info/Elements/u/P60314> ;
    reg:lexicalAlias <http://rdaregistry.info/Elements/m/encodingFormat.en> ;
    reg:name "encodingFormat"@en ;
    reg:status <http://metadataregistry.org/uri/RegStatus/1001> ;
    a rdf:Property ;
    rdfs:domain <http://rdaregistry.info/Elements/c/C10007> ;
    rdfs:isDefinedBy <http://rdaregistry.info/Elements/m/> ;
    rdfs:label "a pour format d’encodage"@fr, "har kodningsformat"@sv, "has encoding format"@en ;
    rdfs:subPropertyOf <http://rdaregistry.info/Elements/m/P30124> ;
    skos:definition "Met une manifestation en relation avec une norme, un schéma, etc. utilisé pour encoder le contenu numérique d’une ressource."@fr, "Relates a manifestation to a schema, standard, etc., used to encode the digital content of a manifestation."@en .

<http://rdaregistry.info/Elements/m/P30097>
    rdakit:instructionNumber "2.6.6" ;
    rdakit:toolkitDefinition "A second or subsequent system of numbering presented in numeric and/or alphabetic form on the first issue or part of a sequence of numbering for a serial."@en, "Deuxième système de numérotation ou système subséquent présenté sous forme numérique et/ou alphabétique sur la première livraison ou la première partie d’une séquence de numérotation d’une publication en série."@fr, "Un segundo o subsecuente sistema de numeración que se presenta en forma numérica y/o alfabética en la primera entrega o parte de una secuencia de numeración para una publicación seriada."@es ;
    rdakit:toolkitLabel "alternativ numerisk och/eller alfabetisk beteckning för första numret/delen i svit"@sv, "alternative numeric and/or alphabetic designation of first issue or part of sequence"@en, "autre indication numérique et/ou alphabétique de la première livraison ou de la première partie de la séquence"@fr, "designación numérica y/o alfabética alternativa de la primera entrega o parte de la secuencia"@es ;
    reg:hasUnconstrained <http://rdaregistry.info/Elements/u/P60820> ;
    reg:lexicalAlias <http://rdaregistry.info/Elements/m/alternativeNumericAndOrAlphabeticDesignationOfFirstIssueOrPartOfSequence.en> ;
    reg:name "alternativeNumericAndOrAlphabeticDesignationOfFirstIssueOrPartOfSequence"@en ;
    reg:status <http://metadataregistry.org/uri/RegStatus/1001> ;
    a rdf:Property ;
    rdfs:domain <http://rdaregistry.info/Elements/c/C10007> ;
    rdfs:isDefinedBy <http://rdaregistry.info/Elements/m/> ;
    rdfs:label "a pour autre indication numérique et/ou alphabétique de la première livraison ou de la première partie de la séquence"@fr, "har alternativ numerisk och/eller alfabetisk beteckning för första numret/delen i svit"@sv, "has alternative numeric and/or alphabetic designation of first issue or part of sequence"@en ;
    rdfs:subPropertyOf <http://rdaregistry.info/Elements/m/P30165> ;
    skos:definition "Met une manifestation en relation avec un deuxième système de numérotation ou un système subséquent présenté sous forme numérique et/ou alphabétique sur la première livraison ou la première partie d’une séquence de numérotation d’une publication en série."@fr, "Relates a manifestation to a second or subsequent system of numbering presented in numeric or alphabetic form on the first issue or part of a sequence of numbering for a serial."@en .

<http://rdaregistry.info/Elements/m/P30098>
    rdakit:instructionNumber "2.6.8" ;
    rdakit:toolkitDefinition "A second or subsequent system of numbering presented in numeric and/or alphabetic form on the last issue or part of a sequence of numbering for a serial."@en, "Deuxième système de numérotation ou système subséquent présenté sous forme numérique et/ou alphabétique sur la dernière livraison ou la dernière partie d’une séquence de numérotation d’une publication en série."@fr, "Un segundo o subsecuente sistema de numeración que se presenta en forma numérica y/o alfabética en la última entrega o parte de una secuencia de numeración para una publicación seriada."@es ;
    rdakit:toolkitLabel "alternativ numerisk och/eller alfabetisk beteckning för sista numret/delen i svit"@sv, "alternative numeric and/or alphabetic designation of last issue or part of sequence"@en, "autre indication numérique et/ou alphabétique de la dernière livraison ou de la dernière partie de la séquence"@fr, "designación numérica y/o alfabética alternativa de la última entrega o parte de la secuencia"@es ;
    reg:hasUnconstrained <http://rdaregistry.info/Elements/u/P60821> ;
    reg:lexicalAlias <http://rdaregistry.info/Elements/m/alternativeNumericAndOrAlphabeticDesignationOfLastIssueOrPartOfSequence.en> ;
    reg:name "alternativeNumericAndOrAlphabeticDesignationOfLastIssueOrPartOfSequence"@en ;
    reg:status <http://metadataregistry.org/uri/RegStatus/1001> ;
    a rdf:Property ;
    rdfs:domain <http://rdaregistry.info/Elements/c/C10007> ;
    rdfs:isDefinedBy <http://rdaregistry.info/Elements/m/> ;
    rdfs:label "a pour autre indication numérique et/ou alphabétique de la dernière livraison ou de la dernière partie de la séquence"@fr, "har alternativ numerisk och/eller alfabetisk beteckning för sista numret/delen i svit"@sv, "has alternative numeric and/or alphabetic designation of last issue or part of sequence"@en ;
    rdfs:subPropertyOf <http://rdaregistry.info/Elements/m/P30165> ;
    skos:definition "Met une manifestation en relation avec un deuxième système de numérotation ou un système subséquent présenté sous forme numérique et/ou alphabétique sur la dernière livraison ou la dernière partie d’une séquence de numérotation d’une publication en série."@fr, "Relates a manifestation to a second or subsequent system of numbering presented in numeric and/or alphabetic form on the last issue or part of a sequence of numbering for a serial."@en .

<http://rdaregistry.info/Elements/m/P30099>
    rdakit:instructionNumber "2.6.7" ;
    rdakit:toolkitDefinition "A second or subsequent system of numbering presented in the form of a date on the first issue or part of a sequence of numbering for a serial."@en, "Deuxième système de numérotation ou système subséquent présenté sous la forme d’une date (par exemple, année ; année et mois ; mois, jour et année) sur la première livraison ou la première partie d’une séquence de numérotation d’une publication en série."@fr, "Un segundo o subsecuente sistema de numeración que se presenta en forma de fecha (por ej., un año; año y mes; mes, día y año) en la primera entrega o parte de una secuencia de numeración para una publicación seriada."@es ;
    rdakit:toolkitLabel "alternative chronological designation of first issue or part of sequence"@en, "autre indication chronologique de la première livraison ou de la première partie de la séquence"@fr, "designación cronológica alternativa de la primera entrega o parte de la secuencia"@es ;
    reg:hasUnconstrained <http://rdaregistry.info/Elements/u/P60818> ;
    reg:lexicalAlias <http://rdaregistry.info/Elements/m/alternativeChronologicalDesignationOfFirstIssueOrPartOfSequence.en> ;
    reg:name "alternativeChronologicalDesignationOfFirstIssueOrPartOfSequence"@en ;
    reg:status <http://metadataregistry.org/uri/RegStatus/1001> ;
    a rdf:Property ;
    rdfs:domain <http://rdaregistry.info/Elements/c/C10007> ;
    rdfs:isDefinedBy <http://rdaregistry.info/Elements/m/> ;
    rdfs:label "a pour autre indication chronologique de la première livraison ou de la première partie de la séquence"@fr, "has alternative chronological designation of first issue or part of sequence"@en ;
    rdfs:subPropertyOf <http://rdaregistry.info/Elements/m/P30165> ;
    skos:definition "Met une manifestation en relation avec un deuxième système de numérotation ou un système subséquent présenté sous la forme d’une date (par exemple, année ; année et mois ; mois, jour et année) sur la première livraison ou la première partie d’une séquence de numérotation d’une publication en série."@fr, "Relates a manifestation to a second or subsequent system of numbering presented in the form of a date on the first issue or part of a sequence of numbering for a serial."@en ;
    skos:scopeNote "Designation includes a year; year and month; month, day, and year. An alternative chronological designation may include a date in a different calendar."@en .

<http://rdaregistry.info/Elements/m/P30100>
    rdakit:instructionNumber "2.6.9" ;
    rdakit:toolkitDefinition "A second or subsequent system of numbering presented in the form of a date on the last issue or part of a sequence of numbering for a serial."@en, "Deuxième système de numérotation ou système subséquent présenté sous la forme d’une date (par exemple, année ; année et mois ; mois, jour et année) sur la dernière livraison ou la dernière partie d’une séquence de numérotation d’une publication en série."@fr, "Un segundo o subsecuente sistema de numeración que se presenta en la forma de fecha (por ej., un año; año y mes; mes, día y año) en la última entrega o parte de una secuencia de numeración para una publicación seriada."@es ;
    rdakit:toolkitLabel "alternative chronological designation of last issue or part of sequence"@en, "autre indication chronologique de la dernière livraison ou de la dernière partie de la séquence"@fr, "designación cronológica alternativa de la última entrega o parte la secuencia"@es ;
    reg:hasUnconstrained <http://rdaregistry.info/Elements/u/P60819> ;
    reg:lexicalAlias <http://rdaregistry.info/Elements/m/alternativeChronologicalDesignationOfLastIssueOrPartOfSequence.en> ;
    reg:name "alternativeChronologicalDesignationOfLastIssueOrPartOfSequence"@en ;
    reg:status <http://metadataregistry.org/uri/RegStatus/1001> ;
    a rdf:Property ;
    rdfs:domain <http://rdaregistry.info/Elements/c/C10007> ;
    rdfs:isDefinedBy <http://rdaregistry.info/Elements/m/> ;
    rdfs:label "a pour autre indication chronologique de la dernière livraison ou de la dernière partie de la séquence"@fr, "has alternative chronological designation of last issue or part of sequence"@en ;
    rdfs:subPropertyOf <http://rdaregistry.info/Elements/m/P30165> ;
    skos:definition "Met une manifestation en relation avec un deuxième système de numérotation ou un système subséquent présenté sous la forme d’une date (par exemple, année ; année et mois ; mois, jour et année) sur la dernière livraison ou la dernière partie d’une séquence de numérotation d’une publication en série."@fr, "Relates a manifestation to a second or subsequent system of numbering presented in the form of a date on the last issue or part of a sequence of numbering for a serial."@en ;
    skos:scopeNote "Designation includes a year; year and month; month, day, and year. An alternative chronological designation may include a date in a different calendar."@en .

<http://rdaregistry.info/Elements/m/P30101>
    rdakit:instructionNumber "24.5" ;
    rdakit:toolkitDefinition "A periodical or newspaper containing a single issue or a supplementary section devoted to a special subject, with or without serial numbering."@en, "Publication en série ou journal contenant un numéro isolé ou un supplément consacré à un sujet spécifique, avec ou sans numérotation, tels qu’un numéro anniversaire d’un périodique ou d’un journal."@fr, "Una publicación seriada o periódico que contiene un número único o sección suplementaria dedicada a un tema especial, con o sin numeración seriada, tal como un número de aniversario de un periódico o revista."@es ;
    rdakit:toolkitLabel "numéro spécial de"@fr, "número especial de"@es, "special issue of"@en ;
    reg:hasSubproperty <http://rdaregistry.info/Elements/m/object/P30101> ;
    reg:hasUnconstrained <http://rdaregistry.info/Elements/u/P60317> ;
    reg:lexicalAlias <http://rdaregistry.info/Elements/m/specialIssueOf.en> ;
    reg:name "specialIssueOf"@en ;
    reg:status <http://metadataregistry.org/uri/RegStatus/1001> ;
    a rdf:Property ;
    rdfs:domain <http://rdaregistry.info/Elements/c/C10007> ;
    rdfs:isDefinedBy <http://rdaregistry.info/Elements/m/> ;
    rdfs:label "est le numéro spécial de"@fr, "is special issue of"@en ;
    rdfs:subPropertyOf <http://rdaregistry.info/Elements/m/P30020> ;
    skos:definition "Met une manifestation en relation avec une publication en série ou un journal contenant un numéro isolé ou un supplément consacré à un sujet spécifique, avec ou sans numérotation, tels qu’un numéro anniversaire d’un périodique ou d’un journal."@fr, "Relates a manifestation to a periodical or newspaper containing a single issue or a supplementary section devoted to a special subject, with or without serial numbering."@en .

<http://rdaregistry.info/Elements/m/P30102>
    rdakit:instructionNumber "3.19.8" ;
    rdakit:toolkitDefinition "A set of technical details relating to the encoding of geospatial information in a manifestation."@en, "Ensemble de détails techniques relatifs à l’encodage de l’information géospatiale dans une ressource cartographique."@fr, "Un conjunto de detalles técnicos relacionados con la codificación de información geoespacial en un recurso cartográfico."@es ;
    rdakit:toolkitLabel "digital representation of cartographic content"@en, "representación digital de contenido cartográfico"@es, "représentation numérique d’un contenu cartographique"@fr ;
    reg:hasUnconstrained <http://rdaregistry.info/Elements/u/P60323> ;
    reg:lexicalAlias <http://rdaregistry.info/Elements/m/digitalRepresentationOfCartographicContent.en> ;
    reg:name "digitalRepresentationOfCartographicContent"@en ;
    reg:status <http://metadataregistry.org/uri/RegStatus/1001> ;
    a rdf:Property ;
    rdfs:domain <http://rdaregistry.info/Elements/c/C10007> ;
    rdfs:isDefinedBy <http://rdaregistry.info/Elements/m/> ;
    rdfs:label "a pour représentation numérique d’un contenu cartographique"@fr, "has digital representation of cartographic content"@en ;
    rdfs:subPropertyOf <http://rdaregistry.info/Elements/m/P30124> ;
    skos:definition "Met une manifestation en relation avec un ensemble de détails techniques relatifs à l’encodage de l’information géospatiale dans une ressource cartographique."@fr, "Relates a manifestation to a set of technical details relating to the encoding of geospatial information in a manifestation."@en .

<http://rdaregistry.info/Elements/m/P30103>
    rdakit:instructionNumber "17.11" ;
    rdakit:toolkitDefinition "A single exemplar or instance of a manifestation."@en, "Exemplaire isolé ou instance d’une manifestation."@fr, "Un ejemplar individual o una instancia de una manifestación."@es ;
    rdakit:toolkitLabel "ejemplar de una manifestación"@es, "exemplaire d’une manifestation"@fr, "exemplar av manifestation"@sv, "exemplar of manifestation"@en ;
    reg:hasSubproperty <http://rdaregistry.info/Elements/m/object/P30103> ;
    reg:lexicalAlias <http://rdaregistry.info/Elements/m/exemplarOfManifestation.en> ;
    reg:name "exemplarOfManifestation"@en ;
    reg:status <http://metadataregistry.org/uri/RegStatus/1001> ;
    a rdf:Property ;
    rdfs:domain <http://rdaregistry.info/Elements/c/C10007> ;
    rdfs:isDefinedBy <http://rdaregistry.info/Elements/m/> ;
    rdfs:label "a pour exemplaire d’une manifestation"@fr, "har exemplar av manifestation"@sv, "has exemplar of manifestation"@en ;
    skos:definition "Met une manifestation en relation avec un exemplaire isolé ou une instance d’une manifestation."@fr, "Relates a manifestation to a single exemplar or instance of a manifestation."@en .

<http://rdaregistry.info/Elements/m/P30104>
    rdakit:instructionNumber "3.18.2" ;
    rdakit:toolkitDefinition "A standard, etc., used to encode the analog video content of a manifestation."@en, "Norme, etc. utilisée pour encoder le contenu vidéo analogique d’une ressource."@fr, "Una norma, etc., utilizada para codificar el contenido de vídeo análogo de un recurso."@es ;
    rdakit:toolkitLabel "format vidéo"@fr, "formato de video"@es, "video format"@en, "videoformat"@sv ;
    reg:hasUnconstrained <http://rdaregistry.info/Elements/u/P60326> ;
    reg:lexicalAlias <http://rdaregistry.info/Elements/m/videoFormat.en> ;
    reg:name "videoFormat"@en ;
    reg:status <http://metadataregistry.org/uri/RegStatus/1001> ;
    a rdf:Property ;
    rdfs:domain <http://rdaregistry.info/Elements/c/C10007> ;
    rdfs:isDefinedBy <http://rdaregistry.info/Elements/m/> ;
    rdfs:label "a pour format vidéo"@fr, "har videoformat"@sv, "has video format"@en ;
    rdfs:subPropertyOf <http://rdaregistry.info/Elements/m/P30126> ;
    skos:definition "Met une manifestation en relation avec une norme, etc. utilisée pour encoder le contenu vidéo analogique d’une ressource."@fr, "Relates a manifestation to a standard, etc., used to encode the analog video content of a manifestation."@en .

<http://rdaregistry.info/Elements/m/P30105>
    rdakit:instructionNumber "2.4.2" ;
    rdakit:toolkitDefinition "A statement associated with a title proper of a manifestation that relates to the identification or function of agents responsible for the creation of, or contribution to the realization of, the intellectual or artistic content of a work."@en, "Mention associée au titre propre d’une ressource et relative à l’identification et/ou la fonction de toute personne, famille ou collectivité responsable de la création, ou ayant contribué à la réalisation du contenu intellectuel ou artistique d’une ressource."@fr, "Una mención asociada con el título propiamente dicho de un recurso que se relaciona con la identificación y/o función de todas las personas, familias, o entidades corporativas responsables de la creación de, o que contribuyen a la realización del contenido intelectual o artístico del recurso."@es ;
    rdakit:toolkitLabel "mención de responsabilidad relacionada con el título propiamente dicho"@es, "mention de responsabilité relative au titre propre"@fr, "parallell upphovsuppgift som hänför sig till huvudtiteln"@sv, "statement of responsibility relating to title proper"@en ;
    reg:hasUnconstrained <http://rdaregistry.info/Elements/u/P60327> ;
    reg:lexicalAlias <http://rdaregistry.info/Elements/m/statementOfResponsibilityRelatingToTitleProper.en> ;
    reg:name "statementOfResponsibilityRelatingToTitleProper"@en ;
    reg:status <http://metadataregistry.org/uri/RegStatus/1001> ;
    a rdf:Property ;
    rdfs:domain <http://rdaregistry.info/Elements/c/C10007> ;
    rdfs:isDefinedBy <http://rdaregistry.info/Elements/m/> ;
    rdfs:label "a pour mention de responsabilité relative au titre propre"@fr, "har parallell upphovsuppgift som hänför sig till huvudtiteln"@sv, "has statement of responsibility relating to title proper"@en ;
    rdfs:subPropertyOf <http://rdaregistry.info/Elements/m/P30117> ;
    skos:definition "Met une manifestation en relation avec une mention associée au titre propre d’une ressource et relative à l’identification et/ou la fonction de toute personne, famille ou collectivité responsable de la création, ou ayant contribué à la réalisation du contenu intellectuel ou artistique d’une ressource."@fr, "Relates a manifestation to a statement associated with a title proper of a manifestation that relates to the identification or function of agents responsible for the creation of, or contribution to the realization of, the intellectual or artistic content of a work."@en .

<http://rdaregistry.info/Elements/m/P30106>
    rdakit:instructionNumber "2.12" ;
    rdakit:toolkitDefinition "A statement identifying a series to which a manifestation belongs and a numbering of a manifestation within the series."@en, "Mention identifiant une collection à laquelle une ressource appartient et la numérotation de la ressource à l’intérieur de la collection."@fr, "Una mención que identifica una serie a la que pertenece un recurso y la numeración del recurso dentro de la serie."@es ;
    rdakit:toolkitLabel "mención de serie"@es, "mention de collection"@fr, "series statement"@en, "serieuppgift"@sv ;
    reg:hasUnconstrained <http://rdaregistry.info/Elements/u/P60328> ;
    reg:lexicalAlias <http://rdaregistry.info/Elements/m/seriesStatement.en> ;
    reg:name "seriesStatement"@en ;
    reg:status <http://metadataregistry.org/uri/RegStatus/1001> ;
    a rdf:Property ;
    rdfs:domain <http://rdaregistry.info/Elements/c/C10007> ;
    rdfs:isDefinedBy <http://rdaregistry.info/Elements/m/> ;
    rdfs:label "a pour mention de collection"@fr, "har serieuppgift"@sv, "has series statement"@en ;
    skos:definition "Met une manifestation en relation avec une mention identifiant une collection à laquelle une ressource appartient et la numérotation de la ressource à l’intérieur de la collection."@fr, "Relates a manifestation to a statement identifying a series to which a manifestation belongs and a numbering of a manifestation within the series."@en ;
    skos:scopeNote "A series statement may also include information identifying one or more subseries to which the resource being described belongs. A series statement sometimes includes statements of responsibility relating to a series or subseries."@en, "Une mention de collection peut aussi comprendre l’information identifiant une ou plusieurs sous-collections auxquelles la ressource décrite appartient. Les mentions de collection comprennent parfois des mentions de responsabilité relatives à une collection ou une sous-collection."@fr .

<http://rdaregistry.info/Elements/m/P30107>
    rdakit:instructionNumber "2.5" ;
    rdakit:toolkitDefinition "A statement identifying an edition to which a manifestation belongs."@en, "Mention identifiant l’édition à laquelle appartient la ressource."@fr, "Una mención que identifica la edición a la que pertenece un recurso."@es ;
    rdakit:toolkitLabel "edition statement"@en, "mención de edición"@es, "mention d’édition"@fr, "upplageuppgift"@sv ;
    reg:hasUnconstrained <http://rdaregistry.info/Elements/u/P60329> ;
    reg:lexicalAlias <http://rdaregistry.info/Elements/m/editionStatement.en> ;
    reg:name "editionStatement"@en ;
    reg:status <http://metadataregistry.org/uri/RegStatus/1001> ;
    a rdf:Property ;
    rdfs:domain <http://rdaregistry.info/Elements/c/C10007> ;
    rdfs:isDefinedBy <http://rdaregistry.info/Elements/m/> ;
    rdfs:label "a pour mention d’édition"@fr, "har upplageuppgift"@sv, "has edition statement"@en ;
    skos:definition "Met une manifestation en relation avec une mention identifiant l’édition à laquelle appartient la ressource."@fr, "Relates a manifestation to a statement identifying an edition to which a manifestation belongs."@en ;
    skos:scopeNote "An edition statement sometimes includes a designation of a named revision of an edition. An edition statement sometimes includes a statement of responsibility relating to the edition or to a named revision of an edition."@en, "Une mention d’édition comprend parfois une indication d’une révision nommée d’une édition. Une mention d’édition comprend parfois une ou plusieurs mentions de responsabilité relatives à l’édition et/ou à une révision nommée d’une édition."@fr .

<http://rdaregistry.info/Elements/m/P30108>
    rdakit:instructionNumber "2.9" ;
    rdakit:toolkitDefinition "A statement identifying a place or places of distribution, distributor or distributors, and date or dates of distribution of a manifestation in a published form."@en, "Mention identifiant le ou les lieux de diffusion ou de distribution, le ou les diffuseurs ou distributeurs et la ou les dates de diffusion ou de distribution d’une ressource sous une forme publiée."@fr, "Una mención que identifica el lugar o lugares de distribución, el distribuidor o distribuidores, y la fecha o fechas de publicación de un recurso en forma publicada."@es ;
    rdakit:toolkitLabel "distribution statement"@en, "distributionsuppgift"@sv, "mención de distribución"@es, "mention de diffusion ou de distribution"@fr ;
    reg:hasUnconstrained <http://rdaregistry.info/Elements/u/P60330> ;
    reg:lexicalAlias <http://rdaregistry.info/Elements/m/distributionStatement.en> ;
    reg:name "distributionStatement"@en ;
    reg:status <http://metadataregistry.org/uri/RegStatus/1001> ;
    a rdf:Property ;
    rdfs:domain <http://rdaregistry.info/Elements/c/C10007> ;
    rdfs:isDefinedBy <http://rdaregistry.info/Elements/m/> ;
    rdfs:label "a pour mention de diffusion ou de distribution"@fr, "har distributionsuppgift"@sv, "has distribution statement"@en ;
    skos:definition "Met une manifestation en relation avec une mention identifiant le ou les lieux de diffusion ou de distribution, le ou les diffuseurs ou distributeurs et la ou les dates de diffusion ou de distribution d’une ressource sous une forme publiée."@fr, "Relates a manifestation to a statement identifying a place or places of distribution, distributor or distributors, and date or dates of distribution of a manifestation in a published form."@en .

<http://rdaregistry.info/Elements/m/P30109>
    rdakit:instructionNumber "2.10" ;
    rdakit:toolkitDefinition "A statement identifying a place or places of manufacture, manufacturer or manufacturers, and date or dates of manufacture of a manifestation in a published form."@en, "Mention identifiant le ou les lieux de fabrication, le ou les fabricants et la ou les dates de fabrication d’une ressource sous une forme publiée."@fr, "Una mención que identifica el lugar o lugares de fabricación, el fabricante o fabricantes, y la fecha o fechas de fabricación de un recurso impreso."@es ;
    rdakit:toolkitLabel "manufacture statement"@en, "mención de fabricación"@es, "mention de fabrication"@fr, "tillverkningsuppgift"@sv ;
    reg:hasUnconstrained <http://rdaregistry.info/Elements/u/P60331> ;
    reg:lexicalAlias <http://rdaregistry.info/Elements/m/manufactureStatement.en> ;
    reg:name "manufactureStatement"@en ;
    reg:status <http://metadataregistry.org/uri/RegStatus/1001> ;
    a rdf:Property ;
    rdfs:domain <http://rdaregistry.info/Elements/c/C10007> ;
    rdfs:isDefinedBy <http://rdaregistry.info/Elements/m/> ;
    rdfs:label "a pour mention de fabrication"@fr, "har tillverkningsuppgift"@sv, "has manufacture statement"@en ;
    skos:definition "Met une manifestation en relation avec une mention identifiant le ou les lieux de fabrication, le ou les fabricants et la ou les dates de fabrication d’une ressource sous une forme publiée."@fr, "Relates a manifestation to a statement identifying a place or places of manufacture, manufacturer or manufacturers, and date or dates of manufacture of a manifestation in a published form."@en ;
    skos:scopeNote "Les mentions de fabrication comprennent les mentions relatives à l’impression, à la reproduction, au moulage, etc. d’une ressource sous une forme publiée."@fr, "Manufacture statements include statements relating to the printing, duplicating, casting, etc., of a manifestation in a published form."@en .

<http://rdaregistry.info/Elements/m/P30110>
    rdakit:instructionNumber "2.7" ;
    rdakit:toolkitDefinition "A statement identifying a place or places of production, producer or producers, and date or dates of production of a manifestation in an unpublished form."@en, "Mention identifiant le ou les lieux de production, le ou les producteurs et la ou les dates de production d’une ressource sous une forme non publiée."@fr, "Una mención que identifica el lugar o lugares de producción, el productor o productores, y la fecha o fechas de producción de un recurso en un formato inédito."@es ;
    rdakit:toolkitLabel "mención de producción"@es, "mention de production"@fr, "production statement"@en, "produktionsuppgift"@sv ;
    reg:hasUnconstrained <http://rdaregistry.info/Elements/u/P60332> ;
    reg:lexicalAlias <http://rdaregistry.info/Elements/m/productionStatement.en> ;
    reg:name "productionStatement"@en ;
    reg:status <http://metadataregistry.org/uri/RegStatus/1001> ;
    a rdf:Property ;
    rdfs:domain <http://rdaregistry.info/Elements/c/C10007> ;
    rdfs:isDefinedBy <http://rdaregistry.info/Elements/m/> ;
    rdfs:label "a pour mention de production"@fr, "har produktionsuppgift"@sv, "has production statement"@en ;
    skos:definition "Met une manifestation en relation avec une mention identifiant le ou les lieux de production, le ou les producteurs et la ou les dates de production d’une ressource sous une forme non publiée."@fr, "Relates a manifestation to a statement identifying a place or places of production, producer or producers, and date or dates of production of a manifestation in an unpublished form."@en ;
    skos:scopeNote "Les mentions de production comprennent les mentions relatives à la scription, à la fabrication, à la construction, etc. d’une ressource sous une forme non publiée."@fr, "Production statements include statements relating to the inscription, fabrication, construction, etc., of a manifestation in an unpublished form."@en .

<http://rdaregistry.info/Elements/m/P30111>
    rdakit:instructionNumber "2.8" ;
    rdakit:toolkitDefinition "A statement identifying a place or places of publication, publisher or publishers, and date or dates of publication of a manifestation."@en, "Mention identifiant le ou les lieux de publication, le ou les éditeurs et la ou les dates de publication d’une ressource."@fr, "Una mención que identifica el lugar o lugares de publicación, el editor o los editores, y la fecha o fechas de publicación de un recurso."@es ;
    rdakit:toolkitLabel "mención de publicación"@es, "mention de publication"@fr, "publication statement"@en, "utgivningsuppgift"@sv ;
    reg:hasUnconstrained <http://rdaregistry.info/Elements/u/P60333> ;
    reg:lexicalAlias <http://rdaregistry.info/Elements/m/publicationStatement.en> ;
    reg:name "publicationStatement"@en ;
    reg:status <http://metadataregistry.org/uri/RegStatus/1001> ;
    a rdf:Property ;
    rdfs:domain <http://rdaregistry.info/Elements/c/C10007> ;
    rdfs:isDefinedBy <http://rdaregistry.info/Elements/m/> ;
    rdfs:label "a pour mention de publication"@fr, "har utgivningsuppgift"@sv, "has publication statement"@en ;
    skos:definition "Met une manifestation en relation avec une mention identifiant le ou les lieux de publication, le ou les éditeurs et la ou les dates de publication d’une ressource."@fr, "Relates a manifestation to a statement identifying a place or places of publication, publisher or publishers, and date or dates of publication of a manifestation."@en ;
    skos:scopeNote "Les mentions de publication comprennent les mentions relatives à la publication, à la mise à disposition ou à l’émission d’une ressource."@fr, "Publication statements include statements relating to the publication, release, or issuing of a manifestation."@en .

<http://rdaregistry.info/Elements/m/P30112>
    rdakit:instructionNumber "2.5.9" ;
    rdakit:toolkitDefinition "A statement of responsibility relating to a named revision of an edition in a language or script that differs from that recorded in a statement of responsibility relating to a named revision of an edition element."@en, "Mention de responsabilité relative à une révision nommée d’une édition dans une langue et/ou une écriture différentes de celles enregistrées dans l’élément Mention de responsabilité relative à une révision nommée d’une édition."@fr, "Una mención de responsabilidad relacionada con una revisión mencionada de una edición en una lengua y/o escritura que difiere de la registrada en la mención de responsabilidad relacionada con el elemento revisión mencionada de una edición."@es ;
    rdakit:toolkitLabel "mención paralela de responsabilidad relacionada con una revisión mencionada de una edición"@es, "mention de responsabilité parallèle relative à une révision nommée d’une édition"@fr, "parallel statement of responsibility relating to named revision of edition"@en, "parallell upphovsuppgift som hänför sig till påföljande upplagebeteckning"@sv ;
    reg:hasUnconstrained <http://rdaregistry.info/Elements/u/P60334> ;
    reg:lexicalAlias <http://rdaregistry.info/Elements/m/parallelStatementOfResponsibilityRelatingToNamedRevisionOfEdition.en> ;
    reg:name "parallelStatementOfResponsibilityRelatingToNamedRevisionOfEdition"@en ;
    reg:status <http://metadataregistry.org/uri/RegStatus/1001> ;
    a rdf:Property ;
    rdfs:domain <http://rdaregistry.info/Elements/c/C10007> ;
    rdfs:isDefinedBy <http://rdaregistry.info/Elements/m/> ;
    rdfs:label "a pour mention de responsabilité parallèle relative à une révision nommée d’une édition"@fr, "har parallell upphovsuppgift som hänför sig till påföljande upplagebeteckning"@sv, "has parallel statement of responsibility relating to named revision of edition"@en ;
    skos:definition "Met une manifestation en relation avec une mention de responsabilité relative à une révision nommée d’une édition dans une langue et/ou une écriture différentes de celles enregistrées dans l’élément Mention de responsabilité relative à une révision nommée d’une édition."@fr, "Relates a manifestation to a statement of responsibility relating to a named revision of an edition in a language or script that differs from that recorded in a statement of responsibility relating to a named revision of an edition element."@en .

<http://rdaregistry.info/Elements/m/P30113>
    rdakit:instructionNumber "2.12.7" ;
    rdakit:toolkitDefinition "A statement of responsibility relating to series in a language or script that differs from that recorded in a statement of responsibility relating to series element."@en, "Mention de responsabilité relative à la collection dans une langue et/ou une écriture différentes de celles enregistrées dans l’élément Mention de responsabilité relative à la collection."@fr, "Una mención de responsabilidad relacionada con la serie en una lengua y/o escritura que difiere de la registrada en el elemento mención de responsabilidad relacionada con la serie."@es ;
    rdakit:toolkitLabel "mención paralela de responsabilidad relacionada con la serie"@es, "mention de responsabilité parallèle relative à la collection"@fr, "parallel statement of responsibility relating to series"@en, "parallell upphovsuppgift till serie"@sv ;
    reg:hasUnconstrained <http://rdaregistry.info/Elements/u/P60335> ;
    reg:lexicalAlias <http://rdaregistry.info/Elements/m/parallelStatementOfResponsibilityRelatingToSeries.en> ;
    reg:name "parallelStatementOfResponsibilityRelatingToSeries"@en ;
    reg:status <http://metadataregistry.org/uri/RegStatus/1001> ;
    a rdf:Property ;
    rdfs:domain <http://rdaregistry.info/Elements/c/C10007> ;
    rdfs:isDefinedBy <http://rdaregistry.info/Elements/m/> ;
    rdfs:label "a pour mention de responsabilité parallèle relative à la collection"@fr, "har parallell upphovsuppgift till serie"@sv, "has parallel statement of responsibility relating to series"@en ;
    skos:definition "Met une manifestation en relation avec une mention de responsabilité relative à la collection dans une langue et/ou une écriture différentes de celles enregistrées dans l’élément Mention de responsabilité relative à la collection."@fr, "Relates a manifestation to a statement of responsibility relating to series in a language or script that differs from that recorded in a statement of responsibility relating to series element."@en .

<http://rdaregistry.info/Elements/m/P30114>
    rdakit:instructionNumber "2.12.15" ;
    rdakit:toolkitDefinition "A statement of responsibility relating to subseries in a language or script that differs from that recorded in a statement of responsibility relating to subseries element."@en, "Mention de responsabilité relative à la sous-collection dans une langue et/ou une écriture différentes de celles enregistrées dans l’élément Mention de responsabilité relative à la sous-collection."@fr, "Una mención de responsabilidad relacionada con una subserie en una lengua y/o escritura que difiere de la registrada en el elemento mención de responsabilidad relacionada con la subserie."@es ;
    rdakit:toolkitLabel "mención paralela de responsabilidad relacionada con la subserie"@es, "mention de responsabilité parallèle relative à la sous-collection"@fr, "parallel statement of responsibility relating to subseries"@en, "parallell upphovsuppgift till underserie"@sv ;
    reg:hasUnconstrained <http://rdaregistry.info/Elements/u/P60336> ;
    reg:lexicalAlias <http://rdaregistry.info/Elements/m/parallelStatementOfResponsibilityRelatingToSubseries.en> ;
    reg:name "parallelStatementOfResponsibilityRelatingToSubseries"@en ;
    reg:status <http://metadataregistry.org/uri/RegStatus/1001> ;
    a rdf:Property ;
    rdfs:domain <http://rdaregistry.info/Elements/c/C10007> ;
    rdfs:isDefinedBy <http://rdaregistry.info/Elements/m/> ;
    rdfs:label "a pour mention de responsabilité parallèle relative à la sous-collection"@fr, "har parallell upphovsuppgift till underserie"@sv, "has parallel statement of responsibility relating to subseries"@en ;
    skos:definition "Met une manifestation en relation avec une mention de responsabilité relative à la sous-collection dans une langue et/ou une écriture différentes de celles enregistrées dans l’élément Mention de responsabilité relative à la sous-collection."@fr, "Relates a manifestation to a statement of responsibility relating to subseries in a language or script that differs from that recorded in a statement of responsibility relating to subseries element."@en .

<http://rdaregistry.info/Elements/m/P30115>
    rdakit:instructionNumber "2.5.5" ;
    rdakit:toolkitDefinition "A statement of responsibility relating to the edition in a language or script that differs from that recorded in a statement of responsibility relating to the edition element."@en, "Mention de responsabilité relative à l’édition dans une langue et/ou une écriture différentes de celles enregistrées dans l’élément Mention de responsabilité relative à l’édition."@fr, "Una mención de responsabilidad relacionada con la edición en una lengua y/o escritura que difiere de la registrada en la mención de responsabilidad relacionada con el elemento edición"@es ;
    rdakit:toolkitLabel "mención paralela de responsabilidad relacionada con la edición"@es, "mention de responsabilité parallèle relative à l’édition"@fr, "parallel statement of responsibility relating to edition"@en, "parallell upphovsuppgift som hänför sig till upplagan"@sv ;
    reg:hasUnconstrained <http://rdaregistry.info/Elements/u/P60337> ;
    reg:lexicalAlias <http://rdaregistry.info/Elements/m/parallelStatementOfResponsibilityRelatingToEdition.en> ;
    reg:name "parallelStatementOfResponsibilityRelatingToEdition"@en ;
    reg:status <http://metadataregistry.org/uri/RegStatus/1001> ;
    a rdf:Property ;
    rdfs:domain <http://rdaregistry.info/Elements/c/C10007> ;
    rdfs:isDefinedBy <http://rdaregistry.info/Elements/m/> ;
    rdfs:label "a pour mention de responsabilité parallèle relative à l’édition"@fr, "har parallell upphovsuppgift som hänför sig till upplagan"@sv, "has parallel statement of responsibility relating to edition"@en ;
    skos:definition "Met une manifestation en relation avec une mention de responsabilité relative à l’édition dans une langue et/ou une écriture différentes de celles enregistrées dans l’élément Mention de responsabilité relative à l’édition."@fr, "Relates a manifestation to a statement of responsibility relating to the edition in a language or script that differs from that recorded in a statement of responsibility relating to the edition element."@en .

<http://rdaregistry.info/Elements/m/P30116>
    rdakit:instructionNumber "2.4.3" ;
    rdakit:toolkitDefinition "A statement of responsibility relating to title proper in a language or script that differs from that recorded in a statement of responsibility relating to title proper element."@en, "Mention de responsabilité relative au titre propre dans une langue et/ou une écriture différentes de celles enregistrées dans l’élément Mention de responsabilité relative au titre propre."@fr, "Una mención de responsabilidad relacionada con el título propiamente dicho en una lengua y/o escritura que difiere de la registrada en la mención de responsabilidad relacionada con el elemento título propiamente dicho."@es ;
    rdakit:toolkitLabel "mención paralela de responsabilidad relacionada con el título propiamente dicho"@es, "mention de responsabilité parallèle relative au titre propre"@fr, "parallel statement of responsibility relating to title proper"@en, "parallell upphovsuppgift som hänför sig till huvudtiteln"@sv ;
    reg:hasUnconstrained <http://rdaregistry.info/Elements/u/P60338> ;
    reg:lexicalAlias <http://rdaregistry.info/Elements/m/parallelStatementOfResponsibilityRelatingToTitleProper.en> ;
    reg:name "parallelStatementOfResponsibilityRelatingToTitleProper"@en ;
    reg:status <http://metadataregistry.org/uri/RegStatus/1001> ;
    a rdf:Property ;
    rdfs:domain <http://rdaregistry.info/Elements/c/C10007> ;
    rdfs:isDefinedBy <http://rdaregistry.info/Elements/m/> ;
    rdfs:label "a pour mention de responsabilité parallèle relative au titre propre"@fr, "har parallell upphovsuppgift som hänför sig till huvudtiteln"@sv, "has parallel statement of responsibility relating to title proper"@en ;
    rdfs:subPropertyOf <http://rdaregistry.info/Elements/m/P30117> ;
    skos:definition "Met une manifestation en relation avec une mention de responsabilité relative au titre propre dans une langue et/ou une écriture différentes de celles enregistrées dans l’élément Mention de responsabilité relative au titre propre."@fr, "Relates a manifestation to a statement of responsibility relating to title proper in a language or script that differs from that recorded in a statement of responsibility relating to title proper element."@en .

<http://rdaregistry.info/Elements/m/P30117>
    rdakit:instructionNumber "2.4" ;
    rdakit:toolkitDefinition "A statement relating to the identification or function of agents responsible for the creation of, or contributing to the realization of, the intellectual or artistic content of a manifestation."@en, "Mention relative à l’identification et/ou la fonction de toute personne, famille ou collectivité responsable de la création, ou ayant contribué à la réalisation du contenu intellectuel ou artistique d’une ressource."@fr, "Una mención relacionada con la identificación y/o función de personas, familias, o entidades corporativas responsables de la creación de, o que contribuyen a la realización del contenido intelectual del recurso."@es ;
    rdakit:toolkitLabel "mención de responsabilidad"@es, "mention de responsabilité"@fr, "statement of responsibility"@en, "upphovsuppgift"@sv ;
    reg:hasSubproperty <http://rdaregistry.info/Elements/m/P30105>, <http://rdaregistry.info/Elements/m/P30116> ;
    reg:hasUnconstrained <http://rdaregistry.info/Elements/u/P60339> ;
    reg:lexicalAlias <http://rdaregistry.info/Elements/m/statementOfResponsibility.en> ;
    reg:name "statementOfResponsibility"@en ;
    reg:status <http://metadataregistry.org/uri/RegStatus/1001> ;
    a rdf:Property ;
    rdfs:domain <http://rdaregistry.info/Elements/c/C10007> ;
    rdfs:isDefinedBy <http://rdaregistry.info/Elements/m/> ;
    rdfs:label "a pour mention de responsabilité"@fr, "har upphovsuppgift"@sv, "has statement of responsibility"@en ;
    skos:definition "Met une manifestation en relation avec une mention relative à l’identification et/ou la fonction de toute personne, famille ou collectivité responsable de la création, ou ayant contribué à la réalisation du contenu intellectuel ou artistique d’une ressource."@fr, "Relates a manifestation to a statement relating to the identification or function of agents responsible for the creation of, or contributing to the realization of, the intellectual or artistic content of a manifestation."@en ;
    skos:scopeNote "A statement of responsibility sometimes includes words or phrases that are neither names nor linking words."@en, "Une mention de responsabilité comprend parfois des mots ou des expressions qui ne sont ni des noms ni des mots de liaison."@fr .

<http://rdaregistry.info/Elements/m/P30118>
    rdakit:instructionNumber "2.5.8" ;
    rdakit:toolkitDefinition "A statement relating to the identification of agents responsible for a named revision of an edition."@en, "Mention relative à l’identification de toute personne, famille ou collectivité responsable de la révision nommée d’une édition."@fr, "Una mención relacionada con la identificación de todas las personas, familias o entidades corporativas responsables de una revisión mencionada de una edición."@es ;
    rdakit:toolkitLabel "mención de responsabilidad relacionada con una revisión mencionada de una edición"@es, "mention de responsabilité relative à une révision nommée d’une édition"@fr, "statement of responsibility relating to named revision of edition"@en, "upphovsuppgift som hänför sig till påföljande upplageuppgift"@sv ;
    reg:hasUnconstrained <http://rdaregistry.info/Elements/u/P60340> ;
    reg:lexicalAlias <http://rdaregistry.info/Elements/m/statementOfResponsibilityRelatingToNamedRevisionOfEdition.en> ;
    reg:name "statementOfResponsibilityRelatingToNamedRevisionOfEdition"@en ;
    reg:status <http://metadataregistry.org/uri/RegStatus/1001> ;
    a rdf:Property ;
    rdfs:domain <http://rdaregistry.info/Elements/c/C10007> ;
    rdfs:isDefinedBy <http://rdaregistry.info/Elements/m/> ;
    rdfs:label "a pour mention de responsabilité relative à une révision nommée d’une édition"@fr, "har upphovsuppgift som hänför sig till påföljande upplageuppgift"@sv, "has statement of responsibility relating to named revision of edition"@en ;
    skos:definition "Met une manifestation en relation avec une mention relative à l’identification de toute personne, famille ou collectivité responsable de la révision nommée d’une édition."@fr, "Relates a manifestation to a statement relating to the identification of agents responsible for a named revision of an edition."@en .

<http://rdaregistry.info/Elements/m/P30119>
    rdakit:instructionNumber "2.12.6" ;
    rdakit:toolkitDefinition "A statement relating to the identification of agents responsible for a series."@en, "Mention relative à l’identification de toute personne, famille ou collectivité responsable d’une collection."@fr, "Una mención relacionada con la identificación de personas, familias o entidades corporativas responsables de una serie."@es ;
    rdakit:toolkitLabel "mención de responsabilidad relacionada con la serie"@es, "mention de responsabilité relative à la collection"@fr, "statement of responsibility relating to series"@en, "upphovsuppgift till serie"@sv ;
    reg:hasUnconstrained <http://rdaregistry.info/Elements/u/P60341> ;
    reg:lexicalAlias <http://rdaregistry.info/Elements/m/statementOfResponsibilityRelatingToSeries.en> ;
    reg:name "statementOfResponsibilityRelatingToSeries"@en ;
    reg:status <http://metadataregistry.org/uri/RegStatus/1001> ;
    a rdf:Property ;
    rdfs:domain <http://rdaregistry.info/Elements/c/C10007> ;
    rdfs:isDefinedBy <http://rdaregistry.info/Elements/m/> ;
    rdfs:label "a pour mention de responsabilité relative à la collection"@fr, "har upphovsuppgift till serie"@sv, "has statement of responsibility relating to series"@en ;
    skos:definition "Met une manifestation en relation avec une mention relative à l’identification de toute personne, famille ou collectivité responsable d’une collection."@fr, "Relates a manifestation to a statement relating to the identification of agents responsible for a series."@en .

<http://rdaregistry.info/Elements/m/P30120>
    rdakit:instructionNumber "2.12.14" ;
    rdakit:toolkitDefinition "A statement relating to the identification of agents responsible for a subseries."@en, "Mention relative à l’identification de toute personne, famille ou collectivité responsable d’une sous-collection."@fr, "Una mención relacionada con la identificación de personas, familias o entidades corporativas responsables por una subserie."@es ;
    rdakit:toolkitLabel "mención de responsabilidad relacionada con la subserie"@es, "mention de responsabilité relative à la sous-collection"@fr, "statement of responsibility relating to subseries"@en, "upphovsuppgift till underserie"@sv ;
    reg:hasUnconstrained <http://rdaregistry.info/Elements/u/P60342> ;
    reg:lexicalAlias <http://rdaregistry.info/Elements/m/statementOfResponsibilityRelatingToSubseries.en> ;
    reg:name "statementOfResponsibilityRelatingToSubseries"@en ;
    reg:status <http://metadataregistry.org/uri/RegStatus/1001> ;
    a rdf:Property ;
    rdfs:domain <http://rdaregistry.info/Elements/c/C10007> ;
    rdfs:isDefinedBy <http://rdaregistry.info/Elements/m/> ;
    rdfs:label "a pour mention de responsabilité relative à la sous-collection"@fr, "har upphovsuppgift till underserie"@sv, "has statement of responsibility relating to subseries"@en ;
    skos:definition "Met une manifestation en relation avec une mention relative à l’identification de toute personne, famille ou collectivité responsable d’une sous-collection."@fr, "Relates a manifestation to a statement relating to the identification of agents responsible for a subseries."@en .

<http://rdaregistry.info/Elements/m/P30121>
    rdakit:instructionNumber "2.5.4" ;
    rdakit:toolkitDefinition "A statement relating to the identification of agents responsible for an edition being described but not to all editions."@en, "Mention relative à l’identification de toute personne, famille ou collectivité responsable de l’édition décrite mais pas de toutes les éditions."@fr, "Una mención relacionada con la identificación de las personas, familias o entidades corporativas responsables de la edición descrita, pero no de todas las ediciones."@es ;
    rdakit:toolkitLabel "mención de responsabilidad relacionada con la edición"@es, "mention de responsabilité relative à l’édition"@fr, "statement of responsibility relating to edition"@en, "upplagespecifik upphovsuppgift"@sv ;
    reg:hasUnconstrained <http://rdaregistry.info/Elements/u/P60343> ;
    reg:lexicalAlias <http://rdaregistry.info/Elements/m/statementOfResponsibilityRelatingToEdition.en> ;
    reg:name "statementOfResponsibilityRelatingToEdition"@en ;
    reg:status <http://metadataregistry.org/uri/RegStatus/1001> ;
    a rdf:Property ;
    rdfs:domain <http://rdaregistry.info/Elements/c/C10007> ;
    rdfs:isDefinedBy <http://rdaregistry.info/Elements/m/> ;
    rdfs:label "a pour mention de responsabilité relative à l’édition"@fr, "har upplagespecifik upphovsuppgift"@sv, "has statement of responsibility relating to edition"@en ;
    skos:definition "Met une manifestation en relation avec une mention relative à l’identification de toute personne, famille ou collectivité responsable de l’édition décrite mais pas de toutes les éditions."@fr, "Relates a manifestation to a statement relating to the identification of agents responsible for an edition being described but not to all editions."@en .

<http://rdaregistry.info/Elements/m/P30122>
    rdakit:instructionNumber "3.7.2" ;
    rdakit:toolkitDefinition "A suspension of light-sensitive chemicals used as a coating on a microfilm or microfiche."@en, "Suspension de produits chimiques photosensibles utilisés comme revêtement sur un microfilm ou une microfiche (par exemple, l’halogénure d’argent)."@fr, "Una suspensión de químicos suaves utilizados como cobertura en un microfilme o una microficha (por ej., haluro de plata)."@es ;
    rdakit:toolkitLabel "emulsion on microfilm and microfiche"@en, "emulsion på mikrofilm och mikrofiche"@sv, "emulsión en microfilme y microficha"@es, "émulsion sur microfilm et microfiche"@fr ;
    reg:hasUnconstrained <http://rdaregistry.info/Elements/u/P60344> ;
    reg:lexicalAlias <http://rdaregistry.info/Elements/m/emulsionOnMicrofilmAndMicrofiche.en> ;
    reg:name "emulsionOnMicrofilmAndMicrofiche"@en ;
    reg:status <http://metadataregistry.org/uri/RegStatus/1001> ;
    a rdf:Property ;
    rdfs:domain <http://rdaregistry.info/Elements/c/C10007> ;
    rdfs:isDefinedBy <http://rdaregistry.info/Elements/m/> ;
    rdfs:label "a pour émulsion sur microfilm et microfiche"@fr, "har emulsion på mikrofilm och mikrofiche"@sv, "has emulsion on microfilm and microfiche"@en ;
    rdfs:subPropertyOf <http://rdaregistry.info/Elements/m/P30084> ;
    skos:definition "Met une manifestation en relation avec une suspension de produits chimiques photosensibles utilisés comme revêtement sur un microfilm ou une microfiche (par exemple, l’halogénure d’argent)."@fr, "Relates a manifestation to a suspension of light-sensitive chemicals used as a coating on a microfilm or microfiche."@en .

<http://rdaregistry.info/Elements/m/P30123>
    rdakit:instructionNumber "3.18.3" ;
    rdakit:toolkitDefinition "A system used to format a manifestation of a video for television broadcast."@en, "Système utilisé pour formater une ressource vidéo pour la télédiffusion."@fr, "Un sistema utilizado para formatear un recurso de vídeo para transmisión por televisión."@es ;
    rdakit:toolkitLabel "broadcast standard"@en, "norma de transmisión"@es, "norme de diffusion"@fr, "sändningsstandard"@sv ;
    reg:hasUnconstrained <http://rdaregistry.info/Elements/u/P60349> ;
    reg:lexicalAlias <http://rdaregistry.info/Elements/m/broadcastStandard.en> ;
    reg:name "broadcastStandard"@en ;
    reg:status <http://metadataregistry.org/uri/RegStatus/1001> ;
    a rdf:Property ;
    rdfs:domain <http://rdaregistry.info/Elements/c/C10007> ;
    rdfs:isDefinedBy <http://rdaregistry.info/Elements/m/> ;
    rdfs:label "a pour norme de diffusion"@fr, "har sändningsstandard"@sv, "has broadcast standard"@en ;
    rdfs:subPropertyOf <http://rdaregistry.info/Elements/m/P30126> ;
    skos:definition "Met une manifestation en relation avec un système utilisé pour formater une ressource vidéo pour la télédiffusion."@fr, "Relates a manifestation to a system used to format a manifestation of a video for television broadcast."@en .

<http://rdaregistry.info/Elements/m/P30124>
    rdakit:instructionNumber "3.19" ;
    rdakit:toolkitDefinition "A technical specification relating to the digital encoding of text, image, audio, video, and other types of data in a manifestation."@en, "Spécification technique relative à l’encodage numérique de texte, d’image, de données audio, vidéo et autres types de données dans une ressource."@fr, "Una especificación técnica relacionada con la codificación digital de un texto, imagen, audio, vídeo y otros tipos de datos en un recurso."@es ;
    rdakit:toolkitLabel "características del archivo digital"@es, "caractéristique du fichier numérique"@fr, "digital file characteristic"@en, "egenskaper för resursens digitala kodning"@sv ;
    reg:hasSubproperty <http://rdaregistry.info/Elements/m/P30006>, <http://rdaregistry.info/Elements/m/P30018>, <http://rdaregistry.info/Elements/m/P30096>, <http://rdaregistry.info/Elements/m/P30102>, <http://rdaregistry.info/Elements/m/P30159>, <http://rdaregistry.info/Elements/m/P30183>, <http://rdaregistry.info/Elements/m/P30202> ;
    reg:hasUnconstrained <http://rdaregistry.info/Elements/u/P60350> ;
    reg:lexicalAlias <http://rdaregistry.info/Elements/m/digitalFileCharacteristic.en> ;
    reg:name "digitalFileCharacteristic"@en ;
    reg:status <http://metadataregistry.org/uri/RegStatus/1001> ;
    a rdf:Property ;
    rdfs:domain <http://rdaregistry.info/Elements/c/C10007> ;
    rdfs:isDefinedBy <http://rdaregistry.info/Elements/m/> ;
    rdfs:label "a pour caractéristique du fichier numérique"@fr, "har egenskaper för resursens digitala kodning"@sv, "has digital file characteristic"@en ;
    skos:definition "Met une manifestation en relation avec une spécification technique relative à l’encodage numérique de texte, d’image, de données audio, vidéo et autres types de données dans une ressource."@fr, "Relates a manifestation to a technical specification relating to the digital encoding of text, image, audio, video, and other types of data in a manifestation."@en .

<http://rdaregistry.info/Elements/m/P30125>
    rdakit:instructionNumber "3.16" ;
    rdakit:toolkitDefinition "A technical specification relating to the encoding of sound in a manifestation."@en, "Spécification technique relative à l’encodage du son dans une ressource."@fr, "Una especificación técnica relacionada con la codificación del sonido en un recurso."@es ;
    rdakit:toolkitLabel "características de sonido"@es, "caractéristique sonore"@fr, "ljudkaraktäristiska"@sv, "sound characteristic"@en ;
    reg:hasSubproperty <http://rdaregistry.info/Elements/m/P30138>, <http://rdaregistry.info/Elements/m/P30161>, <http://rdaregistry.info/Elements/m/P30164>, <http://rdaregistry.info/Elements/m/P30172>, <http://rdaregistry.info/Elements/m/P30184>, <http://rdaregistry.info/Elements/m/P30185>, <http://rdaregistry.info/Elements/m/P30201>, <http://rdaregistry.info/Elements/m/P30206> ;
    reg:hasUnconstrained <http://rdaregistry.info/Elements/u/P60351> ;
    reg:lexicalAlias <http://rdaregistry.info/Elements/m/soundCharacteristic.en> ;
    reg:name "soundCharacteristic"@en ;
    reg:status <http://metadataregistry.org/uri/RegStatus/1001> ;
    a rdf:Property ;
    rdfs:domain <http://rdaregistry.info/Elements/c/C10007> ;
    rdfs:isDefinedBy <http://rdaregistry.info/Elements/m/> ;
    rdfs:label "a pour caractéristique sonore"@fr, "har ljudkaraktäristiska"@sv, "has sound characteristic"@en ;
    skos:definition "Met une manifestation en relation avec une spécification technique relative à l’encodage du son dans une ressource."@fr, "Relates a manifestation to a technical specification relating to the encoding of sound in a manifestation."@en .

<http://rdaregistry.info/Elements/m/P30126>
    rdakit:instructionNumber "3.18" ;
    rdakit:toolkitDefinition "A technical specification relating to the encoding of video images in a manifestation."@en, "Spécification technique relative à l’encodage des images vidéo d’une ressource."@fr, "Una especificación técnica relacionada con la codificación de las imágenes en un recurso."@es ;
    rdakit:toolkitLabel "características de video"@es, "caractéristique vidéo"@fr, "video characteristic"@en, "videokaraktäristika"@sv ;
    reg:hasSubproperty <http://rdaregistry.info/Elements/m/P30104>, <http://rdaregistry.info/Elements/m/P30123> ;
    reg:hasUnconstrained <http://rdaregistry.info/Elements/u/P60352> ;
    reg:lexicalAlias <http://rdaregistry.info/Elements/m/videoCharacteristic.en> ;
    reg:name "videoCharacteristic"@en ;
    reg:status <http://metadataregistry.org/uri/RegStatus/1001> ;
    a rdf:Property ;
    rdfs:domain <http://rdaregistry.info/Elements/c/C10007> ;
    rdfs:isDefinedBy <http://rdaregistry.info/Elements/m/> ;
    rdfs:label "a pour caractéristique vidéo"@fr, "har videokaraktäristika"@sv, "has video characteristic"@en ;
    skos:definition "Met une manifestation en relation avec une spécification technique relative à l’encodage des images vidéo d’une ressource."@fr, "Relates a manifestation to a technical specification relating to the encoding of video images in a manifestation."@en .

<http://rdaregistry.info/Elements/m/P30127>
    rdakit:instructionNumber "3.17" ;
    rdakit:toolkitDefinition "A technical specification relating to the projection of a motion picture film."@en, "Spécification technique relative à la projection d’un film cinématographique."@fr, "Una especificación técnica relacionada con la proyección de un largometraje."@es ;
    rdakit:toolkitLabel "características de proyección de un largometraje"@es, "caractéristique de projection d’un film cinématographique"@fr, "projection characteristic of motion picture film"@en, "projektionskaraktäristika för film"@sv ;
    reg:hasSubproperty <http://rdaregistry.info/Elements/m/P30163>, <http://rdaregistry.info/Elements/m/P30200> ;
    reg:hasUnconstrained <http://rdaregistry.info/Elements/u/P60353> ;
    reg:lexicalAlias <http://rdaregistry.info/Elements/m/projectionCharacteristicOfMotionPictureFilm.en> ;
    reg:name "projectionCharacteristicOfMotionPictureFilm"@en ;
    reg:status <http://metadataregistry.org/uri/RegStatus/1001> ;
    a rdf:Property ;
    rdfs:domain <http://rdaregistry.info/Elements/c/C10007> ;
    rdfs:isDefinedBy <http://rdaregistry.info/Elements/m/> ;
    rdfs:label "a pour caractéristique de projection d’un film cinématographique"@fr, "har projektionskaraktäristika för film"@sv, "has projection characteristic of motion picture film"@en ;
    skos:definition "Met une manifestation en relation avec une spécification technique relative à la projection d’un film cinématographique."@fr, "Relates a manifestation to a technical specification relating to the projection of a motion picture film."@en .

<http://rdaregistry.info/Elements/m/P30128>
    rdakit:instructionNumber "2.3.6" ;
    rdakit:toolkitDefinition "A title associated with a manifestation that differs from a title recorded as a title proper, a parallel title proper, other title information, parallel other title information, earlier title proper, later title proper, key title, or abbreviated title."@en, "Titre associé à une ressource et qui diffère du titre enregistré comme titre propre, titre propre parallèle, complément du titre, complément du titre parallèle, titre propre antérieur, titre propre ultérieur, titre-clé ou titre abrégé."@fr, "Un título asociado con un recurso que difiere de un título registrado como el título propiamente dicho, un título paralelo propiamente dicho, información complementaria del título, información complementaria paralela del título, título anterior propiamente dicho, título posterior propiamente dicho, título clave, o título abreviado."@es ;
    rdakit:toolkitLabel "variant title"@en, "variante de titre"@fr, "variante del título"@es, "varianttitel"@sv ;
    reg:hasUnconstrained <http://rdaregistry.info/Elements/u/P60355> ;
    reg:lexicalAlias <http://rdaregistry.info/Elements/m/variantTitle.en> ;
    reg:name "variantTitle"@en ;
    reg:status <http://metadataregistry.org/uri/RegStatus/1001> ;
    a rdf:Property ;
    rdfs:domain <http://rdaregistry.info/Elements/c/C10007> ;
    rdfs:isDefinedBy <http://rdaregistry.info/Elements/m/> ;
    rdfs:label "a pour variante de titre"@fr, "har varianttitel"@sv, "has variant title"@en ;
    rdfs:subPropertyOf <http://rdaregistry.info/Elements/m/P30134> ;
    skos:definition "Met une manifestation en relation avec un titre associé à une ressource et qui diffère du titre enregistré comme titre propre, titre propre parallèle, complément du titre, complément du titre parallèle, titre propre antérieur, titre propre ultérieur, titre-clé ou titre abrégé."@fr, "Relates a manifestation to a title associated with a manifestation that differs from a title recorded as a title proper, a parallel title proper, other title information, parallel other title information, earlier title proper, later title proper, key title, or abbreviated title."@en .

<http://rdaregistry.info/Elements/m/P30129>
    rdakit:instructionNumber "2.3.8" ;
    rdakit:toolkitDefinition "A title proper appearing on a later issue or part of a multipart monograph or serial that differs from that on the first or earliest issue or part."@en, "Titre propre figurant sur une livraison ou partie ultérieure d’une monographie en plusieurs parties ou d’une publication en série et qui diffère de celui figurant sur la première ou la plus ancienne livraison ou partie."@fr, "Un título propiamente dicho que aparece en una entrega o parte posterior de una monografía en varias partes o publicación seriada que difiere del de la primera o anterior entrega o parte."@es ;
    rdakit:toolkitLabel "efterföljande huvudtitel"@sv, "later title proper"@en, "titre propre ultérieur"@fr, "título propiamente dicho posterior"@es ;
    reg:hasUnconstrained <http://rdaregistry.info/Elements/u/P60357> ;
    reg:lexicalAlias <http://rdaregistry.info/Elements/m/laterTitleProper.en> ;
    reg:name "laterTitleProper"@en ;
    reg:status <http://metadataregistry.org/uri/RegStatus/1001> ;
    a rdf:Property ;
    rdfs:domain <http://rdaregistry.info/Elements/c/C10007> ;
    rdfs:isDefinedBy <http://rdaregistry.info/Elements/m/> ;
    rdfs:label "a pour titre propre ultérieur"@fr, "har efterföljande huvudtitel"@sv, "has later title proper"@en ;
    rdfs:subPropertyOf <http://rdaregistry.info/Elements/m/P30156> ;
    skos:definition "Met une manifestation en relation avec un titre propre figurant sur une livraison ou partie ultérieure d’une monographie en plusieurs parties ou d’une publication en série et qui diffère de celui figurant sur la première ou la plus ancienne livraison ou partie."@fr, "Relates a manifestation to a title proper appearing on a later issue or part of a multipart monograph or serial that differs from that on the first or earliest issue or part."@en .

<http://rdaregistry.info/Elements/m/P30130>
    rdakit:instructionNumber "2.3.7" ;
    rdakit:toolkitDefinition "A title proper appearing on an earlier iteration of an integrating resource that differs from that on the current iteration."@en, "Titre propre figurant sur une itération antérieure d’une ressource intégratrice et qui diffère du titre de l’itération en cours."@fr, "Un título propiamente dicho que aparece en una iteración anterior de un recurso integrable que difiere del que aparece en la iteración actual."@es ;
    rdakit:toolkitLabel "earlier title proper"@en, "föregående huvudtitel"@sv, "titre propre antérieur"@fr, "título propiamente dicho anterior"@es ;
    reg:hasUnconstrained <http://rdaregistry.info/Elements/u/P60358> ;
    reg:lexicalAlias <http://rdaregistry.info/Elements/m/earlierTitleProper.en> ;
    reg:name "earlierTitleProper"@en ;
    reg:status <http://metadataregistry.org/uri/RegStatus/1001> ;
    a rdf:Property ;
    rdfs:domain <http://rdaregistry.info/Elements/c/C10007> ;
    rdfs:isDefinedBy <http://rdaregistry.info/Elements/m/> ;
    rdfs:label "a pour titre propre antérieur"@fr, "har föregående huvudtitel"@sv, "has earlier title proper"@en ;
    rdfs:subPropertyOf <http://rdaregistry.info/Elements/m/P30156> ;
    skos:definition "Met une manifestation en relation avec un titre propre figurant sur une itération antérieure d’une ressource intégratrice et qui diffère du titre de l’itération en cours."@fr, "Relates a manifestation to a title proper appearing on an earlier iteration of an integrating resource that differs from that on the current iteration."@en .

<http://rdaregistry.info/Elements/m/P30131>
    rdakit:instructionNumber "2.3.10" ;
    rdakit:toolkitDefinition "A title that has been abbreviated for purposes of indexing or identification."@en, "Titre qui a été abrégé à des fins d’indexation ou d’identification."@fr, "Un título que ha sido abreviado para efectos de indización o identificación."@es ;
    rdakit:toolkitLabel "abbreviated title"@en, "förkortad titel"@sv, "titre abrégé"@fr, "título abreviado"@es ;
    reg:hasUnconstrained <http://rdaregistry.info/Elements/u/P60359> ;
    reg:lexicalAlias <http://rdaregistry.info/Elements/m/abbreviatedTitle.en> ;
    reg:name "abbreviatedTitle"@en ;
    reg:status <http://metadataregistry.org/uri/RegStatus/1001> ;
    a rdf:Property ;
    rdfs:domain <http://rdaregistry.info/Elements/c/C10007> ;
    rdfs:isDefinedBy <http://rdaregistry.info/Elements/m/> ;
    rdfs:label "a pour titre abrégé"@fr, "har förkortad titel"@sv, "has abbreviated title"@en ;
    rdfs:subPropertyOf <http://rdaregistry.info/Elements/m/P30134> ;
    skos:definition "Met une manifestation en relation avec un titre qui a été abrégé à des fins d’indexation ou d’identification."@fr, "Relates a manifestation to a title that has been abbreviated for purposes of indexing or identification."@en .

<http://rdaregistry.info/Elements/m/P30132>
    rdakit:instructionNumber "2.5.6" ;
    rdakit:toolkitDefinition "A word, character, or group of words or characters, identifying a particular revision of a named edition."@en, "Mot, caractère ou groupe de mots et/ou caractères identifiant une révision particulière d’une édition nommée."@fr, "Una palabra, carácter, o un grupo de palabras y/o caracteres, que identifican una revisión particular de una revisión mencionada de una edición."@es ;
    rdakit:toolkitLabel "designación de una revisión mencionada de una edición"@es, "designation of named revision of edition"@en, "indication d’une révision nommée d’une édition"@fr, "påföljande upplagebeteckning"@sv ;
    reg:hasUnconstrained <http://rdaregistry.info/Elements/u/P60364> ;
    reg:lexicalAlias <http://rdaregistry.info/Elements/m/designationOfNamedRevisionOfEdition.en> ;
    reg:name "designationOfNamedRevisionOfEdition"@en ;
    reg:status <http://metadataregistry.org/uri/RegStatus/1001> ;
    a rdf:Property ;
    rdfs:domain <http://rdaregistry.info/Elements/c/C10007> ;
    rdfs:isDefinedBy <http://rdaregistry.info/Elements/m/> ;
    rdfs:label "a pour indication d’une révision nommée d’une édition"@fr, "har påföljande upplagebeteckning"@sv, "has designation of named revision of edition"@en ;
    skos:definition "Met une manifestation en relation avec un mot, un caractère ou un groupe de mots et/ou caractères identifiant une révision particulière d’une édition nommée."@fr, "Relates a manifestation to a word, character, or group of words or characters, identifying a particular revision of a named edition."@en .

<http://rdaregistry.info/Elements/m/P30133>
    rdakit:instructionNumber "2.5.2" ;
    rdakit:toolkitDefinition "A word, character, or group of words or characters, identifying an edition to which a manifestation belongs."@en, "Mot, caractère ou groupe de mots et/ou caractères identifiant l’édition à laquelle appartient la ressource."@fr, "Una palabra, carácter, o un grupo de palabras y/o caracteres, que identifican la edición a la que pertenece un recurso"@es ;
    rdakit:toolkitLabel "designación de edición"@es, "designation of edition"@en, "indication de l’édition"@fr, "upplagebeteckning"@sv ;
    reg:hasUnconstrained <http://rdaregistry.info/Elements/u/P60365> ;
    reg:lexicalAlias <http://rdaregistry.info/Elements/m/designationOfEdition.en> ;
    reg:name "designationOfEdition"@en ;
    reg:status <http://metadataregistry.org/uri/RegStatus/1001> ;
    a rdf:Property ;
    rdfs:domain <http://rdaregistry.info/Elements/c/C10007> ;
    rdfs:isDefinedBy <http://rdaregistry.info/Elements/m/> ;
    rdfs:label "a pour indication de l’édition"@fr, "har upplagebeteckning"@sv, "has designation of edition"@en ;
    skos:definition "Met une manifestation en relation avec un mot, un caractère ou un groupe de mots et/ou caractères identifiant l’édition à laquelle appartient la ressource."@fr, "Relates a manifestation to a word, character, or group of words or characters, identifying an edition to which a manifestation belongs."@en .

<http://rdaregistry.info/Elements/m/P30134>
    rdakit:instructionNumber "2.3" ;
    rdakit:toolkitDefinition "A word, character, or group of words or characters that names a manifestation or a work embodied in it."@en, "Mot, caractère ou groupe de mots et/ou de caractères qui nomme une ressource ou une œuvre contenue dans cette ressource."@fr, "Una palabra, carácter, o un grupo de palabras y/o caracteres que nombran un recurso o una obra contenida en ella."@es ;
    rdakit:toolkitLabel "titel"@sv, "title"@en, "titre"@fr, "título"@es ;
    reg:hasSubproperty <http://rdaregistry.info/Elements/m/P30128>, <http://rdaregistry.info/Elements/m/P30131>, <http://rdaregistry.info/Elements/m/P30142>, <http://rdaregistry.info/Elements/m/P30151>, <http://rdaregistry.info/Elements/m/P30156>, <http://rdaregistry.info/Elements/m/P30203>, <http://rdaregistry.info/Elements/m/P30209> ;
    reg:hasUnconstrained <http://rdaregistry.info/Elements/u/P60369> ;
    reg:lexicalAlias <http://rdaregistry.info/Elements/m/title.en> ;
    reg:name "title"@en ;
    reg:status <http://metadataregistry.org/uri/RegStatus/1001> ;
    a rdf:Property ;
    rdfs:domain <http://rdaregistry.info/Elements/c/C10007> ;
    rdfs:isDefinedBy <http://rdaregistry.info/Elements/m/> ;
    rdfs:label "a pour titre"@fr, "har titel"@sv, "has title"@en ;
    skos:definition "Met une manifestation en relation avec un mot, un caractère ou un groupe de mots et/ou de caractères qui nomme une ressource ou une œuvre contenue dans cette ressource."@fr, "Relates a manifestation to a word, character, or group of words or characters that names a manifestation or a work embodied in it."@en .

<http://rdaregistry.info/Elements/m/P30135>
    rdakit:instructionNumber "17.8" ;
    rdakit:toolkitDefinition "A work embodied in a manifestation."@en, "L’œuvre matérialisée dans une manifestation."@fr, "Una obra materializada en una manifestación."@es ;
    rdakit:toolkitLabel "manifesterat verk"@sv, "obra manifestada"@es, "work manifested"@en, "œuvre manifestée"@fr ;
    reg:hasSubproperty <http://rdaregistry.info/Elements/m/object/P30135> ;
    reg:lexicalAlias <http://rdaregistry.info/Elements/m/workManifested.en> ;
    reg:name "workManifested"@en ;
    reg:status <http://metadataregistry.org/uri/RegStatus/1001> ;
    a rdf:Property ;
    rdfs:domain <http://rdaregistry.info/Elements/c/C10007> ;
    rdfs:isDefinedBy <http://rdaregistry.info/Elements/m/> ;
    rdfs:label "a pour œuvre manifestée"@fr, "har manifesterat verk"@sv, "has work manifested"@en ;
    skos:definition "Met une manifestation en relation avec l’œuvre matérialisée dans une manifestation."@fr, "Relates a manifestation to a work embodied in a manifestation."@en .

<http://rdaregistry.info/Elements/m/P30136>
    rdakit:instructionNumber "24.5" ;
    rdakit:toolkitDefinition "A manifestation in an analog format that is transferred to a digital format."@en, "Manifestation sur un support analogique qui a été transférée dans un format numérique."@fr, "Una manifestación en un formato analógico que es transferida a un formato digital."@es ;
    rdakit:toolkitLabel "electronic reproduction of (manifestation)"@en, "reproducción electrónica de (manifestación)"@es, "reproduction électronique de (manifestation)"@fr ;
    reg:hasSubproperty <http://rdaregistry.info/Elements/m/object/P30136> ;
    reg:hasUnconstrained <http://rdaregistry.info/Elements/u/P60469> ;
    reg:lexicalAlias <http://rdaregistry.info/Elements/m/electronicReproductionOfManifestation.en> ;
    reg:name "electronicReproductionOfManifestation"@en ;
    reg:status <http://metadataregistry.org/uri/RegStatus/1001> ;
    a rdf:Property ;
    rdfs:domain <http://rdaregistry.info/Elements/c/C10007> ;
    rdfs:isDefinedBy <http://rdaregistry.info/Elements/m/> ;
    rdfs:label "est la reproduction électronique de (manifestation)"@fr, "is electronic reproduction of (manifestation)"@en ;
    rdfs:subPropertyOf <http://rdaregistry.info/Elements/m/P30043> ;
    skos:definition "Met une manifestation en relation avec une manifestation sur un support analogique qui a été transférée dans un format numérique."@fr, "Relates a manifestation to a manifestation in an analog format that is transferred to a digital format."@en .

<http://rdaregistry.info/Elements/m/P30137>
    rdakit:instructionNumber "2.17" ;
    rdakit:toolkitDefinition "A note providing additional information about manifestation attributes."@en, "Annotation fournissant un complément d’information relatif à des attributs de la manifestation."@fr, "Una nota que proporciona información sobre los atributos de la manifestación."@es ;
    rdakit:toolkitLabel "anmärkning om manifestationen"@sv, "nota sobre la manifestación"@es, "note on manifestation"@en, "note relative à la manifestation"@fr ;
    reg:hasSubproperty <http://rdaregistry.info/Elements/m/P30050>, <http://rdaregistry.info/Elements/m/P30051>, <http://rdaregistry.info/Elements/m/P30052>, <http://rdaregistry.info/Elements/m/P30053>, <http://rdaregistry.info/Elements/m/P30054>, <http://rdaregistry.info/Elements/m/P30055>, <http://rdaregistry.info/Elements/m/P30056>, <http://rdaregistry.info/Elements/m/P30057>, <http://rdaregistry.info/Elements/m/P30058>, <http://rdaregistry.info/Elements/m/P30059>, <http://rdaregistry.info/Elements/m/P30062>, <http://rdaregistry.info/Elements/m/P30063>, <http://rdaregistry.info/Elements/m/P30064>, <http://rdaregistry.info/Elements/m/P30260> ;
    reg:hasUnconstrained <http://rdaregistry.info/Elements/u/P60470> ;
    reg:lexicalAlias <http://rdaregistry.info/Elements/m/noteOnManifestation.en> ;
    reg:name "noteOnManifestation"@en ;
    reg:status <http://metadataregistry.org/uri/RegStatus/1001> ;
    a rdf:Property ;
    rdfs:domain <http://rdaregistry.info/Elements/c/C10007> ;
    rdfs:isDefinedBy <http://rdaregistry.info/Elements/m/> ;
    rdfs:label "a pour note relative à la manifestation"@fr, "har anmärkning om manifestationen"@sv, "has note on manifestation"@en ;
    skos:definition "Met une manifestation en relation avec une annotation fournissant un complément d’information relatif à des attributs de la manifestation."@fr, "Relates a manifestation to a note providing additional information about manifestation attributes."@en .

<http://rdaregistry.info/Elements/m/P30138>
    rdakit:instructionNumber "3.16.9" ;
    rdakit:toolkitDefinition "An equalization system, noise reduction system, etc., used in making an audio recording."@en, "Système d’égalisation, de réduction du bruit, etc. utilisé pour fabriquer un enregistrement audio."@fr, "Un sistema de ecualización, sistema de reducción del sonido, etc., utilizado en la producción de una grabación de sonido."@es ;
    rdakit:toolkitLabel "características especiales de reproducción"@es, "caractéristique de lecture particulière"@fr, "special playback characteristic"@en, "specifika uppspelningskaraktäristika"@sv ;
    reg:hasUnconstrained <http://rdaregistry.info/Elements/u/P60481> ;
    reg:lexicalAlias <http://rdaregistry.info/Elements/m/specialPlaybackCharacteristic.en> ;
    reg:name "specialPlaybackCharacteristic"@en ;
    reg:status <http://metadataregistry.org/uri/RegStatus/1001> ;
    a rdf:Property ;
    rdfs:domain <http://rdaregistry.info/Elements/c/C10007> ;
    rdfs:isDefinedBy <http://rdaregistry.info/Elements/m/> ;
    rdfs:label "a pour caractéristique de lecture particulière"@fr, "har specifika uppspelningskaraktäristika"@sv, "has special playback characteristic"@en ;
    rdfs:subPropertyOf <http://rdaregistry.info/Elements/m/P30125> ;
    skos:definition "Met une manifestation en relation avec un système d’égalisation, de réduction du bruit, etc. utilisé pour fabriquer un enregistrement audio."@fr, "Relates a manifestation to an equalization system, noise reduction system, etc., used in making an audio recording."@en .

<http://rdaregistry.info/Elements/m/P30139>
    rdakit:instructionNumber "17.10" ;
    rdakit:toolkitDefinition "An expression embodied in a manifestation."@en, "Expression matérialisée dans une manifestation."@fr, "Una expresión materializada en una manifestación."@es ;
    rdakit:toolkitLabel "expresión manifestada"@es, "expression manifested"@en, "expression manifestée"@fr, "manifesterat uttryck"@sv ;
    reg:hasSubproperty <http://rdaregistry.info/Elements/m/object/P30139> ;
    reg:lexicalAlias <http://rdaregistry.info/Elements/m/expressionManifested.en> ;
    reg:name "expressionManifested"@en ;
    reg:status <http://metadataregistry.org/uri/RegStatus/1001> ;
    a rdf:Property ;
    rdfs:domain <http://rdaregistry.info/Elements/c/C10007> ;
    rdfs:isDefinedBy <http://rdaregistry.info/Elements/m/> ;
    rdfs:label "a pour expression manifestée"@fr, "har manifesterat uttryck"@sv, "has expression manifested"@en ;
    skos:definition "Met une manifestation en relation avec une expression matérialisée dans une manifestation."@fr, "Relates a manifestation to an expression embodied in a manifestation."@en .

<http://rdaregistry.info/Elements/m/P30140>
    rdakit:toolkitDefinition "Item associé à la ressource décrite (par exemple, item utilisé comme base d’une reproduction microforme)."@fr, "Un ítem, representado por un identificador o una descripción, que está relacionada con el recurso que se describe (p.ej., un ítem utilizado como base para una reproducción de una microforma)."@es ;
    rdakit:toolkitLabel "item en relation"@fr, "relaterat exemplar"@sv, "ítem relacionado"@es ;
    reg:hasSubproperty <http://rdaregistry.info/Elements/m/datatype/P30140>, <http://rdaregistry.info/Elements/m/object/P30140> ;
    reg:hasUnconstrained <http://rdaregistry.info/Elements/u/P60313> ;
    reg:lexicalAlias <http://rdaregistry.info/Elements/m/relatedItemManifestation.en> ;
    reg:name "relatedItemManifestation"@en ;
    reg:status <http://metadataregistry.org/uri/RegStatus/1001> ;
    a rdf:Property ;
    rdfs:domain <http://rdaregistry.info/Elements/c/C10007> ;
    rdfs:isDefinedBy <http://rdaregistry.info/Elements/m/> ;
    rdfs:label "a pour item en relation"@fr, "har relaterat exemplar"@sv, "has related item (manifestation)"@en ;
    rdfs:subPropertyOf <http://rdaregistry.info/Elements/m/P30264> ;
    skos:definition "Met une manifestation en relation avec un item associé à la ressource décrite (par exemple, item utilisé comme base d’une reproduction microforme)."@fr, "Relates a manifestation to an item associated with a manifestation being described."@en .

<http://rdaregistry.info/Elements/m/P30141>
    rdakit:instructionNumber "4.3" ;
    rdakit:toolkitDefinition "A name, address, etc., of an organization, etc., from which a manifestation may be obtained."@en, "Información sobre la organización, etc., de la cual se puede obtener un recurso."@es, "Renseignements sur une organisation, etc. auprès de laquelle une ressource peut être obtenue."@fr ;
    rdakit:toolkitLabel "contact information"@en, "coordonnées"@fr, "información de contacto"@es, "kontaktinformation"@sv ;
    reg:hasUnconstrained <http://rdaregistry.info/Elements/u/P60490> ;
    reg:lexicalAlias <http://rdaregistry.info/Elements/m/contactInformation.en> ;
    reg:name "contactInformation"@en ;
    reg:status <http://metadataregistry.org/uri/RegStatus/1001> ;
    a rdf:Property ;
    rdfs:domain <http://rdaregistry.info/Elements/c/C10007> ;
    rdfs:isDefinedBy <http://rdaregistry.info/Elements/m/> ;
    rdfs:label "a pour coordonnées"@fr, "har kontaktinformation"@sv, "has contact information"@en ;
    skos:definition "Met une manifestation en relation avec des renseignements sur une organisation, etc. auprès de laquelle une ressource peut être obtenue."@fr, "Relates a manifestation to a name, address, etc., of an organization, etc., from which a manifestation may be obtained."@en ;
    skos:scopeNote "Contact information includes a name, address, etc. of the publisher, distributor, etc. of a published manifestation, or of the archival repository that holds the manifestation."@en .

<http://rdaregistry.info/Elements/m/P30142>
    rdakit:instructionNumber "2.3.4" ;
    rdakit:toolkitDefinition "A word, character, or group of words or characters that appears in conjunction with, and is subordinate to, a title proper of a manifestation."@en, "Información que aparece en conjunción con el título, y está subordinada al título propiamente dicho de un recurso."@es, "Information reliée et subordonnée au titre propre d’une ressource."@fr ;
    rdakit:toolkitLabel "complément du titre"@fr, "información complementaria del título"@es, "other title information"@en, "övrig titelinformation"@sv ;
    reg:hasUnconstrained <http://rdaregistry.info/Elements/u/P60493> ;
    reg:lexicalAlias <http://rdaregistry.info/Elements/m/otherTitleInformation.en> ;
    reg:name "otherTitleInformation"@en ;
    reg:status <http://metadataregistry.org/uri/RegStatus/1001> ;
    a rdf:Property ;
    rdfs:domain <http://rdaregistry.info/Elements/c/C10007> ;
    rdfs:isDefinedBy <http://rdaregistry.info/Elements/m/> ;
    rdfs:label "a pour complément du titre"@fr, "har övrig titelinformation"@sv, "has other title information"@en ;
    rdfs:subPropertyOf <http://rdaregistry.info/Elements/m/P30134> ;
    skos:definition "Met une manifestation en relation avec une information reliée et subordonnée au titre propre d’une ressource."@fr, "Relates a manifestation to a word, character, or group of words or characters that appears in conjunction with, and is subordinate to, a title proper of a manifestation."@en .

<http://rdaregistry.info/Elements/m/P30143>
    rdakit:instructionNumber "2.12.4" ;
    rdakit:toolkitDefinition "A word, character, or group of words or characters that appears in conjunction with, and is subordinate to, a title proper of a series."@en, "Información que aparece en conjunción con el título propiamente dicho de una serie y está subordinada a él."@es, "Information reliée et subordonnée au titre propre d’une collection."@fr ;
    rdakit:toolkitLabel "complément du titre de collection"@fr, "información complementaria del título de la serie"@es, "other title information of series"@en, "övrig titelinformation för serie"@sv ;
    reg:hasUnconstrained <http://rdaregistry.info/Elements/u/P60494> ;
    reg:lexicalAlias <http://rdaregistry.info/Elements/m/otherTitleInformationOfSeries.en> ;
    reg:name "otherTitleInformationOfSeries"@en ;
    reg:status <http://metadataregistry.org/uri/RegStatus/1001> ;
    a rdf:Property ;
    rdfs:domain <http://rdaregistry.info/Elements/c/C10007> ;
    rdfs:isDefinedBy <http://rdaregistry.info/Elements/m/> ;
    rdfs:label "a pour complément du titre de collection"@fr, "har övrig titelinformation för serie"@sv, "has other title information of series"@en ;
    skos:definition "Met une manifestation en relation avec une information reliée et subordonnée au titre propre d’une collection."@fr, "Relates a manifestation to a word, character, or group of words or characters that appears in conjunction with, and is subordinate to, a title proper of a series."@en .

<http://rdaregistry.info/Elements/m/P30144>
    rdakit:instructionNumber "2.12.12" ;
    rdakit:toolkitDefinition "A word, character, or group of words or characters that appears in conjunction with, and is subordinate to, a title proper of a subseries."@en, "Información que aparece en conjunción con el título propiamente dicho de una subserie y está subordinada a él."@es, "Information reliée et subordonnée au titre propre d’une sous-collection."@fr ;
    rdakit:toolkitLabel "complément du titre de sous-collection"@fr, "información complementaria del título de la subserie"@es, "other title information of subseries"@en, "övrig titelinformation för underserie"@sv ;
    reg:hasUnconstrained <http://rdaregistry.info/Elements/u/P60495> ;
    reg:lexicalAlias <http://rdaregistry.info/Elements/m/otherTitleInformationOfSubseries.en> ;
    reg:name "otherTitleInformationOfSubseries"@en ;
    reg:status <http://metadataregistry.org/uri/RegStatus/1001> ;
    a rdf:Property ;
    rdfs:domain <http://rdaregistry.info/Elements/c/C10007> ;
    rdfs:isDefinedBy <http://rdaregistry.info/Elements/m/> ;
    rdfs:label "a pour complément du titre de sous-collection"@fr, "har övrig titelinformation för underserie"@sv, "has other title information of subseries"@en ;
    skos:definition "Met une manifestation en relation avec une information reliée et subordonnée au titre propre d’une sous-collection."@fr, "Relates a manifestation to a word, character, or group of words or characters that appears in conjunction with, and is subordinate to, a title proper of a subseries."@en .

<http://rdaregistry.info/Elements/m/P30145>
    rdakit:instructionNumber "4.4" ;
    rdakit:toolkitDefinition "A limitation placed on access to a manifestation."@en, "Limitaciones establecidas para el acceso a un recurso."@es, "Limitations imposées sur l’accès à une ressource."@fr ;
    rdakit:toolkitLabel "restricciones de acceso"@es, "restriction on access to manifestation"@en, "restrictions d’accès"@fr, "åtkomstrestriktioner"@sv ;
    reg:hasUnconstrained <http://rdaregistry.info/Elements/u/P60496> ;
    reg:lexicalAlias <http://rdaregistry.info/Elements/m/restrictionOnAccessToManifestation.en> ;
    reg:name "restrictionOnAccessToManifestation"@en ;
    reg:status <http://metadataregistry.org/uri/RegStatus/1001> ;
    a rdf:Property ;
    rdfs:domain <http://rdaregistry.info/Elements/c/C10007> ;
    rdfs:isDefinedBy <http://rdaregistry.info/Elements/m/> ;
    rdfs:label "a pour restrictions d’accès"@fr, "har åtkomstrestriktioner"@sv, "has restriction on access to manifestation"@en ;
    skos:definition "Met une manifestation en relation avec des limitations imposées sur l’accès à une ressource."@fr, "Relates a manifestation to a limitation placed on access to a manifestation."@en .

<http://rdaregistry.info/Elements/m/P30146>
    rdakit:instructionNumber "4.5" ;
    rdakit:toolkitDefinition "A limitation placed on reproduction, publication, exhibition, etc., of a manifestation."@en, "Limitaciones establecidas sobre los usos, tales como reproducción, publicación, exhibición, etc."@es, "Limitations imposées sur des usages tels que la reproduction, la publication, l’exposition, etc."@fr ;
    rdakit:toolkitLabel "användningsrestriktioner"@sv, "restricciones sobre el uso"@es, "restriction on use of manifestation"@en, "restrictions d’usage"@fr ;
    reg:hasUnconstrained <http://rdaregistry.info/Elements/u/P60497> ;
    reg:lexicalAlias <http://rdaregistry.info/Elements/m/restrictionOnUseOfManifestation.en> ;
    reg:name "restrictionOnUseOfManifestation"@en ;
    reg:status <http://metadataregistry.org/uri/RegStatus/1001> ;
    a rdf:Property ;
    rdfs:domain <http://rdaregistry.info/Elements/c/C10007> ;
    rdfs:isDefinedBy <http://rdaregistry.info/Elements/m/> ;
    rdfs:label "a pour restrictions d’usage"@fr, "har användningsrestriktioner"@sv, "has restriction on use of manifestation"@en ;
    skos:definition "Met une manifestation en relation avec des limitations imposées sur des usages tels que la reproduction, la publication, l’exposition, etc."@fr, "Relates a manifestation to a limitation placed on reproduction, publication, exhibition, etc., of a manifestation."@en .

<http://rdaregistry.info/Elements/m/P30147>
    rdakit:instructionNumber "2.6.2" ;
    rdakit:toolkitDefinition "A designation in numeric and/or alphabetic form presented on the first issue or part of a serial issued in a sequence of numbering."@en, "Numeración presentada en forma numérica y/o alfabética en la primera entrega o parte de una secuencia de numeración de una publicación seriada."@es, "Numérotation présentée sous une forme numérique et/ou alphabétique sur la première livraison ou partie d’une séquence de numérotation pour une publication en série."@fr ;
    rdakit:toolkitLabel "designación numérica y/o alfabética de la primera entrega o parte de la secuencia"@es, "indication numérique et/ou alphabétique de la première livraison ou de la première partie de la séquence"@fr, "numeric and/or alphabetic designation of first issue or part of sequence"@en, "numerisk och/eller alfabetisk beteckning för första numret/delen i svit"@sv ;
    reg:hasUnconstrained <http://rdaregistry.info/Elements/u/P60499> ;
    reg:lexicalAlias <http://rdaregistry.info/Elements/m/numericAndOrAlphabeticDesignationOfFirstIssueOrPartOfSequence.en> ;
    reg:name "numericAndOrAlphabeticDesignationOfFirstIssueOrPartOfSequence"@en ;
    reg:status <http://metadataregistry.org/uri/RegStatus/1001> ;
    a rdf:Property ;
    rdfs:domain <http://rdaregistry.info/Elements/c/C10007> ;
    rdfs:isDefinedBy <http://rdaregistry.info/Elements/m/> ;
    rdfs:label "a pour indication numérique et/ou alphabétique de la première livraison ou de la première partie de la séquence"@fr, "har numerisk och/eller alfabetisk beteckning för första numret/delen i svit"@sv, "has numeric and/or alphabetic designation of first issue or part of sequence"@en ;
    rdfs:subPropertyOf <http://rdaregistry.info/Elements/m/P30165> ;
    skos:definition "Met une manifestation en relation avec une numérotation présentée sous une forme numérique et/ou alphabétique sur la première livraison ou partie d’une séquence de numérotation pour une publication en série."@fr, "Relates a manifestation to a designation in numeric and/or alphabetic form presented on the first issue or part of a serial issued in a sequence of numbering."@en .

<http://rdaregistry.info/Elements/m/P30148>
    rdakit:instructionNumber "2.6.4" ;
    rdakit:toolkitDefinition "A designation in numeric and/or alphabetic form presented on the last issue or part of a serial issued in a sequence of numbering."@en, "Numeración presentada en forma numérica y/o alfabética en la última entrega o parte de una secuencia de numeración de una publicación seriada."@es, "Numérotation présentée sous une forme numérique et/ou alphabétique sur la dernière livraison ou partie d’une séquence de numérotation pour une publication en série."@fr ;
    rdakit:toolkitLabel "designación numérica y/o alfabética de la última entrega o parte de la secuencia"@es, "indication numérique et/ou alphabétique de la dernière livraison ou de la dernière partie de la séquence"@fr, "numeric and/or alphabetic designation of last issue or part of sequence"@en, "numerisk och/eller alfabetisk beteckning för sista numret/delen i svit"@sv ;
    reg:hasUnconstrained <http://rdaregistry.info/Elements/u/P60500> ;
    reg:lexicalAlias <http://rdaregistry.info/Elements/m/numericAndOrAlphabeticDesignationOfLastIssueOrPartOfSequence.en> ;
    reg:name "numericAndOrAlphabeticDesignationOfLastIssueOrPartOfSequence"@en ;
    reg:status <http://metadataregistry.org/uri/RegStatus/1001> ;
    a rdf:Property ;
    rdfs:domain <http://rdaregistry.info/Elements/c/C10007> ;
    rdfs:isDefinedBy <http://rdaregistry.info/Elements/m/> ;
    rdfs:label "a pour indication numérique et/ou alphabétique de la dernière livraison ou de la dernière partie de la séquence"@fr, "har numerisk och/eller alfabetisk beteckning för sista numret/delen i svit"@sv, "has numeric and/or alphabetic designation of last issue or part of sequence"@en ;
    rdfs:subPropertyOf <http://rdaregistry.info/Elements/m/P30165> ;
    skos:definition "Met une manifestation en relation avec une numérotation présentée sous une forme numérique et/ou alphabétique sur la dernière livraison ou partie d’une séquence de numérotation pour une publication en série."@fr, "Relates a manifestation to a designation in numeric and/or alphabetic form presented on the last issue or part of a serial issued in a sequence of numbering."@en .

<http://rdaregistry.info/Elements/m/P30149>
    rdakit:instructionNumber "2.6.3" ;
    rdakit:toolkitDefinition "A designation in date form presented on the first issue or part of a serial issued in a sequence of numbering."@en, "Numeración presentada en forma de fecha (por ej., un año; año y mes; mes, día, y año) en la primera entrega o parte de una secuencia de numeración de una publicación seriada."@es, "Numérotation présentée sous la forme d’une date (par exemple, année ; année et mois ; mois, jour et année) sur la première livraison ou la première partie d’une séquence de numérotation d’une publication en série."@fr ;
    rdakit:toolkitLabel "chronological designation of first issue or part of sequence"@en, "designación cronológica de la primera entrega o parte de la secuencia"@es, "indication chronologique de la première livraison ou de la première partie de la séquence"@fr ;
    reg:hasUnconstrained <http://rdaregistry.info/Elements/u/P60501> ;
    reg:lexicalAlias <http://rdaregistry.info/Elements/m/chronologicalDesignationOfFirstIssueOrPartOfSequence.en> ;
    reg:name "chronologicalDesignationOfFirstIssueOrPartOfSequence"@en ;
    reg:status <http://metadataregistry.org/uri/RegStatus/1001> ;
    a rdf:Property ;
    rdfs:domain <http://rdaregistry.info/Elements/c/C10007> ;
    rdfs:isDefinedBy <http://rdaregistry.info/Elements/m/> ;
    rdfs:label "a pour indication chronologique de la première livraison ou de la première partie de la séquence"@fr, "has chronological designation of first issue or part of sequence"@en ;
    rdfs:subPropertyOf <http://rdaregistry.info/Elements/m/P30165> ;
    skos:definition "Met une manifestation en relation avec une numérotation présentée sous la forme d’une date (par exemple, année ; année et mois ; mois, jour et année) sur la première livraison ou la première partie d’une séquence de numérotation d’une publication en série."@fr, "Relates a manifestation to a designation in date form presented on the first issue or part of a serial issued in a sequence of numbering."@en ;
    skos:scopeNote "Designation includes a year; year and month; month, day, and year."@en .

<http://rdaregistry.info/Elements/m/P30150>
    rdakit:instructionNumber "2.6.5" ;
    rdakit:toolkitDefinition "A designation in date form presented on the last issue or part of a serial issued in a sequence of numbering."@en, "Numeración presentada en forma de fecha (por ej., un año; año y mes; mes, día y año) en la última entrega o parte de una secuencia de numeración de una publicación seriada."@es, "Numérotation présentée sous la forme d’une date (par exemple, année ; année et mois ; mois, jour et année) sur la dernière livraison ou la dernière partie d’une séquence de numérotation d’une publication en série."@fr ;
    rdakit:toolkitLabel "chronological designation of last issue or part of sequence"@en, "designación cronológica de la última entrega o parte de la secuencia"@es, "indication chronologique de la dernière livraison ou de la dernière partie de la séquence"@fr ;
    reg:hasUnconstrained <http://rdaregistry.info/Elements/u/P60502> ;
    reg:lexicalAlias <http://rdaregistry.info/Elements/m/chronologicalDesignationOfLastIssueOrPartOfSequence.en> ;
    reg:name "chronologicalDesignationOfLastIssueOrPartOfSequence"@en ;
    reg:status <http://metadataregistry.org/uri/RegStatus/1001> ;
    a rdf:Property ;
    rdfs:domain <http://rdaregistry.info/Elements/c/C10007> ;
    rdfs:isDefinedBy <http://rdaregistry.info/Elements/m/> ;
    rdfs:label "a pour indication chronologique de la dernière livraison ou de la dernière partie de la séquence"@fr, "has chronological designation of last issue or part of sequence"@en ;
    rdfs:subPropertyOf <http://rdaregistry.info/Elements/m/P30165> ;
    skos:definition "Met une manifestation en relation avec une numérotation présentée sous la forme d’une date (par exemple, année ; année et mois ; mois, jour et année) sur la dernière livraison ou la dernière partie d’une séquence de numérotation d’une publication en série."@fr, "Relates a manifestation to a designation in date form presented on the last issue or part of a serial issued in a sequence of numbering."@en ;
    skos:scopeNote "Designation includes a year; year and month; month, day, and year."@en .

<http://rdaregistry.info/Elements/m/P30151>
    rdakit:instructionNumber "2.3.5" ;
    rdakit:toolkitDefinition "An other title information in a language or script that differs from that recorded in an other title information element."@en, "Complément du titre dans une langue et/ou une écriture différentes de celles enregistrées dans l’élément Complément du titre."@fr, "Información complementaria del título en una lengua y/o escritura que difiere de la registrada en el elemento información complementaria del título."@es ;
    rdakit:toolkitLabel "complément du titre parallèle"@fr, "información complementaria paralela del título"@es, "parallel other title information"@en, "parallell övrig titelinformation"@sv ;
    reg:hasUnconstrained <http://rdaregistry.info/Elements/u/P60507> ;
    reg:lexicalAlias <http://rdaregistry.info/Elements/m/parallelOtherTitleInformation.en> ;
    reg:name "parallelOtherTitleInformation"@en ;
    reg:status <http://metadataregistry.org/uri/RegStatus/1001> ;
    a rdf:Property ;
    rdfs:domain <http://rdaregistry.info/Elements/c/C10007> ;
    rdfs:isDefinedBy <http://rdaregistry.info/Elements/m/> ;
    rdfs:label "a pour complément du titre parallèle"@fr, "har parallell övrig titelinformation"@sv, "has parallel other title information"@en ;
    rdfs:subPropertyOf <http://rdaregistry.info/Elements/m/P30134> ;
    skos:definition "Met une manifestation en relation avec un complément du titre dans une langue et/ou une écriture différentes de celles enregistrées dans l’élément Complément du titre."@fr, "Relates a manifestation to an other title information in a language or script that differs from that recorded in an other title information element."@en .

<http://rdaregistry.info/Elements/m/P30152>
    rdakit:instructionNumber "2.12.5" ;
    rdakit:toolkitDefinition "An other title information of a series in a language or script that differs from that recorded in an other title information of series element."@en, "Complément du titre d’une collection dans une langue et/ou une écriture différentes de celles enregistrées dans l’élément Complément du titre d’une collection."@fr, "Información sobre el título de una serie en una lengua y/o escritura que difiere de la registrada en el elemento información complementaria del título de la serie."@es ;
    rdakit:toolkitLabel "complément du titre parallèle d’une collection"@fr, "información complementaria paralela del título de la serie"@es, "parallel other title information of series"@en, "parallell övrig titelinformation för serie"@sv ;
    reg:hasUnconstrained <http://rdaregistry.info/Elements/u/P60508> ;
    reg:lexicalAlias <http://rdaregistry.info/Elements/m/parallelOtherTitleInformationOfSeries.en> ;
    reg:name "parallelOtherTitleInformationOfSeries"@en ;
    reg:status <http://metadataregistry.org/uri/RegStatus/1001> ;
    a rdf:Property ;
    rdfs:domain <http://rdaregistry.info/Elements/c/C10007> ;
    rdfs:isDefinedBy <http://rdaregistry.info/Elements/m/> ;
    rdfs:label "a pour complément du titre parallèle d’une collection"@fr, "har parallell övrig titelinformation för serie"@sv, "has parallel other title information of series"@en ;
    skos:definition "Met une manifestation en relation avec un complément du titre d’une collection dans une langue et/ou une écriture différentes de celles enregistrées dans l’élément Complément du titre d’une collection."@fr, "Relates a manifestation to an other title information of a series in a language or script that differs from that recorded in an other title information of series element."@en .

<http://rdaregistry.info/Elements/m/P30153>
    rdakit:instructionNumber "2.12.13" ;
    rdakit:toolkitDefinition "An other title information of a subseries in a language or script that differs from that recorded in an other title information of subseries element."@en, "Complément du titre d’une sous-collection dans une langue et/ou une écriture différentes de celles enregistrées dans l’élément Complément du titre d’une sous-collection."@fr, "Información complementaria de una subserie en una lengua y/o escritura que difiere de la registrada en el elemento información complementaria del título de la subserie."@es ;
    rdakit:toolkitLabel "complément du titre parallèle d’une sous-collection"@fr, "información complementaria paralela del título de la subserie"@es, "parallel other title information of subseries"@en, "parallell övrig titelinformation för underserie"@sv ;
    reg:hasUnconstrained <http://rdaregistry.info/Elements/u/P60509> ;
    reg:lexicalAlias <http://rdaregistry.info/Elements/m/parallelOtherTitleInformationOfSubseries.en> ;
    reg:name "parallelOtherTitleInformationOfSubseries"@en ;
    reg:status <http://metadataregistry.org/uri/RegStatus/1001> ;
    a rdf:Property ;
    rdfs:domain <http://rdaregistry.info/Elements/c/C10007> ;
    rdfs:isDefinedBy <http://rdaregistry.info/Elements/m/> ;
    rdfs:label "a pour complément du titre parallèle d’une sous-collection"@fr, "har parallell övrig titelinformation för underserie"@sv, "has parallel other title information of subseries"@en ;
    skos:definition "Met une manifestation en relation avec un complément du titre d’une sous-collection dans une langue et/ou une écriture différentes de celles enregistrées dans l’élément Complément du titre d’une sous-collection."@fr, "Relates a manifestation to an other title information of a subseries in a language or script that differs from that recorded in an other title information of subseries element."@en .

<http://rdaregistry.info/Elements/m/P30154>
    rdakit:instructionNumber "4.6" ;
    rdakit:toolkitDefinition "An address of an online resource."@en, "La dirección de un recurso de acceso remoto."@es, "L’adresse d’une ressource accessible en ligne."@fr ;
    rdakit:toolkitLabel "Localizador Uniforme de Recurso"@es, "URL"@sv, "Uniform Resource Locator"@en, "adresse URL"@fr ;
    reg:hasUnconstrained <http://rdaregistry.info/Elements/u/P60511> ;
    reg:lexicalAlias <http://rdaregistry.info/Elements/m/uniformResourceLocator.en> ;
    reg:name "uniformResourceLocator"@en ;
    reg:status <http://metadataregistry.org/uri/RegStatus/1001> ;
    a rdf:Property ;
    rdfs:domain <http://rdaregistry.info/Elements/c/C10007> ;
    rdfs:isDefinedBy <http://rdaregistry.info/Elements/m/> ;
    rdfs:label "a pour adresse URL"@fr, "har URL"@sv, "has uniform resource locator"@en ;
    skos:altLabel "URL"@en ;
    skos:definition "Met une manifestation en relation avec l’adresse d’une ressource accessible en ligne."@fr, "Relates a manifestation to an address of an online resource."@en ;
    skos:scopeNote "A Uniform Resource Locator includes all manifestation identifiers intended to provide online access to a manifestation using a standard Internet browser."@en .

<http://rdaregistry.info/Elements/m/P30155>
    rdakit:instructionNumber "3.11" ;
    rdakit:toolkitDefinition "An arrangement of text, images, tactile notation, etc., in a manifestation."@en, "El arreglo del texto, imágenes, notación táctil, etc., en un recurso."@es, "L’agencement du texte, des images, etc. dans une ressource."@fr ;
    rdakit:toolkitLabel "disposition"@fr, "layout"@en, "layout"@sv, "presentación"@es ;
    reg:hasUnconstrained <http://rdaregistry.info/Elements/u/P60513> ;
    reg:lexicalAlias <http://rdaregistry.info/Elements/m/layout.en> ;
    reg:name "layout"@en ;
    reg:status <http://metadataregistry.org/uri/RegStatus/1001> ;
    a rdf:Property ;
    rdfs:domain <http://rdaregistry.info/Elements/c/C10007> ;
    rdfs:isDefinedBy <http://rdaregistry.info/Elements/m/> ;
    rdfs:label "a pour disposition"@fr, "har layout"@sv, "has layout"@en ;
    skos:definition "Met une manifestation en relation avec l’agencement du texte, des images, etc. dans une ressource."@fr, "Relates a manifestation to an arrangement of text, images, tactile notation, etc., in a manifestation."@en .

<http://rdaregistry.info/Elements/m/P30156>
    rdakit:instructionNumber "2.3.2" ;
    rdakit:toolkitDefinition "A chief name of a manifestation, that is, a title normally used when naming a manifestation."@en, "El nombre principal de un recurso (i.e., el título normalmente usado para citar el recurso)."@es, "Le titre principal d’une ressource (c’est-à-dire le titre normalement utilisé pour citer la ressource)."@fr ;
    rdakit:toolkitLabel "huvudtitel"@sv, "title proper"@en, "titre propre"@fr, "título propiamente dicho"@es ;
    reg:hasUnconstrained <http://rdaregistry.info/Elements/u/P60515> ;
    reg:lexicalAlias <http://rdaregistry.info/Elements/m/titleProper.en> ;
    reg:name "titleProper"@en ;
    reg:status <http://metadataregistry.org/uri/RegStatus/1001> ;
    a rdf:Property ;
    rdfs:domain <http://rdaregistry.info/Elements/c/C10007> ;
    rdfs:isDefinedBy <http://rdaregistry.info/Elements/m/> ;
    rdfs:label "a pour titre propre"@fr, "har huvudtitel"@sv, "has title proper"@en ;
    rdfs:subPropertyOf <http://rdaregistry.info/Elements/m/P30134> ;
    skos:definition "Met une manifestation en relation avec le titre principal d’une ressource (c’est-à-dire le titre normalement utilisé pour citer la ressource)."@fr, "Relates a manifestation to a chief name of a manifestation, that is, a title normally used when naming a manifestation."@en ;
    skos:scopeNote "An alternative title is treated as part of a title proper."@en .

<http://rdaregistry.info/Elements/m/P30157>
    rdakit:instructionNumber "2.12.2" ;
    rdakit:toolkitDefinition "A name of a series appearing on a manifestation of a part of a series."@en, "El nombre principal de la serie (i.e., el título normalmente usado para citar la serie)."@es, "Le titre principal d’une collection (c’est-à-dire le titre normalement utilisé pour citer la collection)."@fr ;
    rdakit:toolkitLabel "huvudtitel till serie"@sv, "title proper of series"@en, "titre propre de la collection"@fr, "título propiamente dicho de la serie"@es ;
    reg:hasUnconstrained <http://rdaregistry.info/Elements/u/P60516> ;
    reg:lexicalAlias <http://rdaregistry.info/Elements/m/titleProperOfSeries.en> ;
    reg:name "titleProperOfSeries"@en ;
    reg:status <http://metadataregistry.org/uri/RegStatus/1001> ;
    a rdf:Property ;
    rdfs:domain <http://rdaregistry.info/Elements/c/C10007> ;
    rdfs:isDefinedBy <http://rdaregistry.info/Elements/m/> ;
    rdfs:label "a pour titre propre de la collection"@fr, "har huvudtitel till serie"@sv, "has title proper of series"@en ;
    skos:definition "Met une manifestation en relation avec le titre principal d’une collection (c’est-à-dire le titre normalement utilisé pour citer la collection)."@fr, "Relates a manifestation to a name of a series appearing on a manifestation of a part of a series."@en .

<http://rdaregistry.info/Elements/m/P30158>
    rdakit:instructionNumber "2.12.10" ;
    rdakit:toolkitDefinition "A name of a series appearing on a manifestation of a part of a subseries."@en, "El nombre principal de la subserie (i.e., el título normalmente usado para citar la subserie)."@es, "Le titre principal d’une sous-collection (c’est-à-dire le titre normalement utilisé pour citer la sous-collection)."@fr ;
    rdakit:toolkitLabel "huvudtitel till underserie"@sv, "title proper of subseries"@en, "titre propre de la sous-collection"@fr, "título propiamente dicho de la subserie"@es ;
    reg:hasUnconstrained <http://rdaregistry.info/Elements/u/P60517> ;
    reg:lexicalAlias <http://rdaregistry.info/Elements/m/titleProperOfSubseries.en> ;
    reg:name "titleProperOfSubseries"@en ;
    reg:status <http://metadataregistry.org/uri/RegStatus/1001> ;
    a rdf:Property ;
    rdfs:domain <http://rdaregistry.info/Elements/c/C10007> ;
    rdfs:isDefinedBy <http://rdaregistry.info/Elements/m/> ;
    rdfs:label "a pour titre propre de la sous-collection"@fr, "har huvudtitel till underserie"@sv, "has title proper of subseries"@en ;
    skos:definition "Met une manifestation en relation avec le titre principal d’une sous-collection (c’est-à-dire le titre normalement utilisé pour citer la sous-collection)."@fr, "Relates a manifestation to a name of a series appearing on a manifestation of a part of a subseries."@en .

<http://rdaregistry.info/Elements/m/P30159>
    rdakit:instructionNumber "3.19.5" ;
    rdakit:toolkitDefinition "A clarity or fineness of detail in a digital image, expressed by the measurement of the image in pixels, etc."@en, "La claridad o exactitud del detalle en una imagen digital, expresada por la medida de la imagen en pixeles, etc."@es, "La netteté ou la finesse de détail d’une image numérique, exprimée par la mesure de l’image en pixels, etc."@fr ;
    rdakit:toolkitLabel "resolución"@es, "resolution"@en, "résolution"@fr, "upplösning"@sv ;
    reg:hasUnconstrained <http://rdaregistry.info/Elements/u/P60519> ;
    reg:lexicalAlias <http://rdaregistry.info/Elements/m/resolution.en> ;
    reg:name "resolution"@en ;
    reg:status <http://metadataregistry.org/uri/RegStatus/1001> ;
    a rdf:Property ;
    rdfs:domain <http://rdaregistry.info/Elements/c/C10007> ;
    rdfs:isDefinedBy <http://rdaregistry.info/Elements/m/> ;
    rdfs:label "a pour résolution"@fr, "har upplösning"@sv, "has resolution"@en ;
    rdfs:subPropertyOf <http://rdaregistry.info/Elements/m/P30124> ;
    skos:definition "Met une manifestation en relation avec la netteté ou la finesse de détail d’une image numérique, exprimée par la mesure de l’image en pixels, etc."@fr, "Relates a manifestation to a clarity or fineness of detail in a digital image, expressed by the measurement of the image in pixels, etc."@en .

<http://rdaregistry.info/Elements/m/P30160>
    rdakit:instructionNumber "4.2" ;
    rdakit:toolkitDefinition "A condition under which the publisher, distributor, etc., will normally supply a manifestation or the price of a manifestation."@en, "Las condiciones bajo las cuales el editor, distribuidor, etc., normalmente ofrecerá un recurso o el precio del recurso."@es, "Les conditions auxquelles l’éditeur, le diffuseur ou le distributeur, etc. fournit normalement une ressource ou bien le prix d’une ressource."@fr ;
    rdakit:toolkitLabel "anskaffningsvillkor"@sv, "modalités d’acquisition"@fr, "term of availability"@en, "términos de disponibilidad"@es ;
    reg:hasUnconstrained <http://rdaregistry.info/Elements/u/P60521> ;
    reg:lexicalAlias <http://rdaregistry.info/Elements/m/termOfAvailability.en> ;
    reg:name "termOfAvailability"@en ;
    reg:status <http://metadataregistry.org/uri/RegStatus/1001> ;
    a rdf:Property ;
    rdfs:domain <http://rdaregistry.info/Elements/c/C10007> ;
    rdfs:isDefinedBy <http://rdaregistry.info/Elements/m/> ;
    rdfs:label "a pour modalités d’acquisition"@fr, "har anskaffningsvillkor"@sv, "has term of availability"@en ;
    skos:definition "Met une manifestation en relation avec les conditions auxquelles l’éditeur, le diffuseur ou le distributeur, etc. fournit normalement une ressource ou bien le prix d’une ressource."@fr, "Relates a manifestation to a condition under which the publisher, distributor, etc., will normally supply a manifestation or the price of a manifestation."@en .

<http://rdaregistry.info/Elements/m/P30161>
    rdakit:instructionNumber "3.16.6" ;
    rdakit:toolkitDefinition "A configuration of the audio track on a sound-track film."@en, "La configuración de la banda de sonido en una película de banda sonora (por ej., pista central)."@es, "La configuration de la piste audio sur la bande sonore d’un film (par exemple, piste centrale)."@fr ;
    rdakit:toolkitLabel "configuración de banda sonora"@es, "configuration de piste"@fr, "ljudspårskonfiguration för film"@sv, "track configuration"@en ;
    reg:hasUnconstrained <http://rdaregistry.info/Elements/u/P60522> ;
    reg:lexicalAlias <http://rdaregistry.info/Elements/m/trackConfiguration.en> ;
    reg:name "trackConfiguration"@en ;
    reg:status <http://metadataregistry.org/uri/RegStatus/1001> ;
    a rdf:Property ;
    rdfs:domain <http://rdaregistry.info/Elements/c/C10007> ;
    rdfs:isDefinedBy <http://rdaregistry.info/Elements/m/> ;
    rdfs:label "a pour configuration de piste"@fr, "har ljudspårskonfiguration för film"@sv, "has track configuration"@en ;
    rdfs:subPropertyOf <http://rdaregistry.info/Elements/m/P30125> ;
    skos:definition "Met une manifestation en relation avec la configuration de la piste audio sur la bande sonore d’un film (par exemple, piste centrale)."@fr, "Relates a manifestation to a configuration of the audio track on a sound-track film."@en .

<http://rdaregistry.info/Elements/m/P30162>
    rdakit:instructionNumber "3.20" ;
    rdakit:toolkitDefinition "A system or equipment required for use, playback, etc., of an analog, digital, etc., manifestation."@en, "El equipo o sistema requerido para usar, reproducir, etc., un recurso análogo, digital, etc."@es, "L’équipement ou le système nécessaire pour l’utilisation, la lecture, etc. d’une ressource analogique, numérique, etc."@fr ;
    rdakit:toolkitLabel "equipment or system requirement"@en, "requerimientos de equipo o sistema"@es, "utrustning eller systemkrav"@sv, "équipement ou système requis"@fr ;
    reg:hasUnconstrained <http://rdaregistry.info/Elements/u/P60528> ;
    reg:lexicalAlias <http://rdaregistry.info/Elements/m/equipmentOrSystemRequirement.en> ;
    reg:name "equipmentOrSystemRequirement"@en ;
    reg:status <http://metadataregistry.org/uri/RegStatus/1001> ;
    a rdf:Property ;
    rdfs:domain <http://rdaregistry.info/Elements/c/C10007> ;
    rdfs:isDefinedBy <http://rdaregistry.info/Elements/m/> ;
    rdfs:label "a pour équipement ou système requis"@fr, "har utrustning eller systemkrav"@sv, "has equipment or system requirement"@en ;
    skos:definition "Met une manifestation en relation avec l’équipement ou le système nécessaire pour l’utilisation, la lecture, etc. d’une ressource analogique, numérique, etc."@fr, "Relates a manifestation to a system or equipment required for use, playback, etc., of an analog, digital, etc., manifestation."@en .

<http://rdaregistry.info/Elements/m/P30163>
    rdakit:instructionNumber "3.17.2" ;
    rdakit:toolkitDefinition "A format used in the production of a projected image."@en, "El formato utilizado en la producción de una imagen proyectada (por ej., Cinerama, IMAX)."@es, "Le format utilisé pour la production d’une image projetée (par exemple, Cinérama, IMAX)."@fr ;
    rdakit:toolkitLabel "filmprojektionssystem"@sv, "formato de presentación"@es, "presentation format"@en, "procédé de projection"@fr ;
    reg:hasUnconstrained <http://rdaregistry.info/Elements/u/P60529> ;
    reg:lexicalAlias <http://rdaregistry.info/Elements/m/presentationFormat.en> ;
    reg:name "presentationFormat"@en ;
    reg:status <http://metadataregistry.org/uri/RegStatus/1001> ;
    a rdf:Property ;
    rdfs:domain <http://rdaregistry.info/Elements/c/C10007> ;
    rdfs:isDefinedBy <http://rdaregistry.info/Elements/m/> ;
    rdfs:label "a pour procédé de projection"@fr, "har filmprojektionssystem"@sv, "has presentation format"@en ;
    rdfs:subPropertyOf <http://rdaregistry.info/Elements/m/P30127> ;
    skos:definition "Met une manifestation en relation avec le format utilisé pour la production d’une image projetée (par exemple, Cinérama, IMAX)."@fr, "Relates a manifestation to a format used in the production of a projected image."@en .

<http://rdaregistry.info/Elements/m/P30164>
    rdakit:instructionNumber "3.16.5" ;
    rdakit:toolkitDefinition "A groove width of an analog disc or a groove pitch of an analog cylinder."@en, "La amplitud del surco de un disco análogo o el tono del surco de un cilindro análogo."@es, "La largeur de sillon d’un disque analogique ou le pas du sillon d’un cylindre analogique."@fr ;
    rdakit:toolkitLabel "características del surco"@es, "caractéristique de sillon"@fr, "groove characteristic"@en, "spårkarakteristika"@sv ;
    reg:hasUnconstrained <http://rdaregistry.info/Elements/u/P60532> ;
    reg:lexicalAlias <http://rdaregistry.info/Elements/m/grooveCharacteristic.en> ;
    reg:name "grooveCharacteristic"@en ;
    reg:status <http://metadataregistry.org/uri/RegStatus/1001> ;
    a rdf:Property ;
    rdfs:domain <http://rdaregistry.info/Elements/c/C10007> ;
    rdfs:isDefinedBy <http://rdaregistry.info/Elements/m/> ;
    rdfs:label "a pour caractéristique de sillon"@fr, "har spårkarakteristika"@sv, "has groove characteristic"@en ;
    rdfs:subPropertyOf <http://rdaregistry.info/Elements/m/P30125> ;
    skos:definition "Met une manifestation en relation avec la largeur de sillon d’un disque analogique ou le pas du sillon d’un cylindre analogique."@fr, "Relates a manifestation to a groove width of an analog disc or a groove pitch of an analog cylinder."@en .

<http://rdaregistry.info/Elements/m/P30165>
    rdakit:instructionNumber "2.6" ;
    rdakit:toolkitDefinition "A designation for each of the issues or parts of a serial."@en, "La identificación de cada una de las entregas o partes de una publicación seriada."@es, "L’identification de chacune des livraisons ou parties d’une publication en série."@fr ;
    rdakit:toolkitLabel "numbering of serials"@en, "numeración de publicaciones seriadas"@es, "numrering av seriella resurser"@sv, "numérotation des publications en série"@fr ;
    reg:hasSubproperty <http://rdaregistry.info/Elements/m/P30097>, <http://rdaregistry.info/Elements/m/P30098>, <http://rdaregistry.info/Elements/m/P30099>, <http://rdaregistry.info/Elements/m/P30100>, <http://rdaregistry.info/Elements/m/P30147>, <http://rdaregistry.info/Elements/m/P30148>, <http://rdaregistry.info/Elements/m/P30149>, <http://rdaregistry.info/Elements/m/P30150> ;
    reg:hasUnconstrained <http://rdaregistry.info/Elements/u/P60533> ;
    reg:lexicalAlias <http://rdaregistry.info/Elements/m/numberingOfSerials.en> ;
    reg:name "numberingOfSerials"@en ;
    reg:status <http://metadataregistry.org/uri/RegStatus/1001> ;
    a rdf:Property ;
    rdfs:domain <http://rdaregistry.info/Elements/c/C10007> ;
    rdfs:isDefinedBy <http://rdaregistry.info/Elements/m/> ;
    rdfs:label "a pour numérotation des publications en série"@fr, "har numrering av seriella resurser"@sv, "has numbering of serials"@en ;
    skos:definition "Met une manifestation en relation avec l’identification de chacune des livraisons ou parties d’une publication en série."@fr, "Relates a manifestation to a designation for each of the issues or parts of a serial."@en ;
    skos:scopeNote "La numérotation des publications en série peut comprendre un chiffre, une lettre, tout autre caractère ou la combinaison de ces éléments, accompagnés ou non d’une appellation (volume, numéro, etc.) et/ou d’une indication chronologique"@fr, "Numbering includes a numeral, a letter, any other character, or the combination of these with or without an accompanying caption and/or a chronological designation."@en .

<http://rdaregistry.info/Elements/m/P30166>
    rdakit:instructionNumber "2.12.8" ;
    rdakit:toolkitDefinition "An identifier assigned to a series by an ISSN registration agency."@en, "El identificador asignado a una serie por una agencia de registro del ISSN."@es, "L’identifiant attribué à une collection par une agence d’enregistrement de l’ISSN."@fr ;
    rdakit:toolkitLabel "ISSN de collection"@fr, "ISSN de series"@es, "ISSN of series"@en, "series ISSN"@sv ;
    reg:hasUnconstrained <http://rdaregistry.info/Elements/u/P60534> ;
    reg:lexicalAlias <http://rdaregistry.info/Elements/m/issnOfSeries.en> ;
    reg:name "issnOfSeries"@en ;
    reg:status <http://metadataregistry.org/uri/RegStatus/1001> ;
    a rdf:Property ;
    rdfs:domain <http://rdaregistry.info/Elements/c/C10007> ;
    rdfs:isDefinedBy <http://rdaregistry.info/Elements/m/> ;
    rdfs:label "a pour ISSN de collection"@fr, "har series ISSN"@sv, "has ISSN of series"@en ;
    skos:definition "Met une manifestation en relation avec l’identifiant attribué à une collection par une agence d’enregistrement de l’ISSN."@fr, "Relates a manifestation to an identifier assigned to a series by an ISSN registration agency."@en .

<http://rdaregistry.info/Elements/m/P30167>
    rdakit:instructionNumber "2.12.16" ;
    rdakit:toolkitDefinition "An identifier assigned to a subseries by an ISSN registration agency."@en, "El identificador asignado a una subserie por una agencia de registro del ISSN."@es, "L’identifiant attribué à une sous-collection par une agence d’enregistrement de l’ISSN."@fr ;
    rdakit:toolkitLabel "ISSN de la subserie"@es, "ISSN de sous-collection"@fr, "ISSN of subseries"@en, "underseries ISSN"@sv ;
    reg:hasUnconstrained <http://rdaregistry.info/Elements/u/P60535> ;
    reg:lexicalAlias <http://rdaregistry.info/Elements/m/issnOfSubseries.en> ;
    reg:name "issnOfSubseries"@en ;
    reg:status <http://metadataregistry.org/uri/RegStatus/1001> ;
    a rdf:Property ;
    rdfs:domain <http://rdaregistry.info/Elements/c/C10007> ;
    rdfs:isDefinedBy <http://rdaregistry.info/Elements/m/> ;
    rdfs:label "a pour ISSN de sous-collection"@fr, "har underseries ISSN"@sv, "has ISSN of subseries"@en ;
    skos:definition "Met une manifestation en relation avec l’identifiant attribué à une sous-collection par une agence d’enregistrement de l’ISSN."@fr, "Relates a manifestation to an identifier assigned to a subseries by an ISSN registration agency."@en .

<http://rdaregistry.info/Elements/m/P30168>
    rdakit:instructionNumber "2.14" ;
    rdakit:toolkitDefinition "An interval at which an issue or part of a serial or an update to an integrating resource is issued."@en, "El intervalo en el cual se editan las entregas o partes de una publicación seriada o las actualizaciones de un recurso integrado."@es, "Les intervalles de temps suivant lesquels les livraisons ou parties d’une publication en série ou les mises à jour d’une ressource intégratrice sont publiées."@fr ;
    rdakit:toolkitLabel "frecuencia"@es, "frequency"@en, "périodicité"@fr, "utgivningsfrekvens"@sv ;
    reg:hasUnconstrained <http://rdaregistry.info/Elements/u/P60538> ;
    reg:lexicalAlias <http://rdaregistry.info/Elements/m/frequency.en> ;
    reg:name "frequency"@en ;
    reg:status <http://metadataregistry.org/uri/RegStatus/1001> ;
    a rdf:Property ;
    rdfs:domain <http://rdaregistry.info/Elements/c/C10007> ;
    rdfs:isDefinedBy <http://rdaregistry.info/Elements/m/> ;
    rdfs:label "a pour périodicité"@fr, "har utgivningsfrekvens"@sv, "has frequency"@en ;
    skos:definition "Met une manifestation en relation avec les intervalles de temps suivant lesquels les livraisons ou parties d’une publication en série ou les mises à jour d’une ressource intégratrice sont publiées."@fr, "Relates a manifestation to an interval at which an issue or part of a serial or an update to an integrating resource is issued."@en .

<http://rdaregistry.info/Elements/m/P30169>
    rdakit:instructionNumber "3.5" ;
    rdakit:toolkitDefinition "A measurement of a carrier or a container of a manifestation."@en, "Las medidas del soporte o soportes y/o el envase de un recurso."@es, "Les mesures du ou des supports matériels et/ou du conteneur d’une ressource."@fr ;
    rdakit:toolkitLabel "dimensiones"@es, "dimensions"@en, "dimensions"@fr, "mått"@sv ;
    reg:hasSubproperty <http://rdaregistry.info/Elements/m/P30170>, <http://rdaregistry.info/Elements/m/P30171> ;
    reg:hasUnconstrained <http://rdaregistry.info/Elements/u/P60539> ;
    reg:lexicalAlias <http://rdaregistry.info/Elements/m/dimensions.en> ;
    reg:name "dimensions"@en ;
    reg:status <http://metadataregistry.org/uri/RegStatus/1001> ;
    a rdf:Property ;
    rdfs:domain <http://rdaregistry.info/Elements/c/C10007> ;
    rdfs:isDefinedBy <http://rdaregistry.info/Elements/m/> ;
    rdfs:label "a pour dimensions"@fr, "har mått"@sv, "has dimensions"@en ;
    skos:definition "Met une manifestation en relation avec les mesures du ou des supports matériels et/ou du conteneur d’une ressource."@fr, "Relates a manifestation to a measurement of a carrier or a container of a manifestation."@en ;
    skos:scopeNote "Dimensions include measurements of height, width, depth, length, gauge, and diameter."@en, "Les dimensions comprennent les mesures de hauteur, de largeur, de profondeur, de longueur et de diamètre ainsi que le format."@fr .

<http://rdaregistry.info/Elements/m/P30170>
    rdakit:instructionNumber "3.5.2" ;
    rdakit:toolkitDefinition "A measurement of a face of a map, etc."@en, "Las medidas de la cara de un mapa, etc."@es, "Les mesures de la surface d’une carte, etc."@fr ;
    rdakit:toolkitLabel "dimensiones del mapa, etc."@es, "dimensions d’une carte, etc."@fr, "dimensions of map, etc."@en, "mått på kartor etc."@sv ;
    reg:hasUnconstrained <http://rdaregistry.info/Elements/u/P60540> ;
    reg:lexicalAlias <http://rdaregistry.info/Elements/m/dimensionsOfMapEtc.en> ;
    reg:name "dimensionsOfMapEtc"@en ;
    reg:status <http://metadataregistry.org/uri/RegStatus/1001> ;
    a rdf:Property ;
    rdfs:domain <http://rdaregistry.info/Elements/c/C10007> ;
    rdfs:isDefinedBy <http://rdaregistry.info/Elements/m/> ;
    rdfs:label "a pour dimensions d’une carte, etc."@fr, "har mått på kartor etc."@sv, "has dimensions of map, etc."@en ;
    rdfs:subPropertyOf <http://rdaregistry.info/Elements/m/P30169> ;
    skos:definition "Met une manifestation en relation avec les mesures de la surface d’une carte, etc."@fr, "Relates a manifestation to a measurement of a face of a map, etc."@en .

<http://rdaregistry.info/Elements/m/P30171>
    rdakit:instructionNumber "3.5.3" ;
    rdakit:toolkitDefinition "A measurement of the pictorial area of a still image."@en, "La medidas del área pictórica de una imagen fija."@es, "Les mesures de la partie graphique d’une image fixe."@fr ;
    rdakit:toolkitLabel "bildytans mått"@sv, "dimensiones de la imagen fija"@es, "dimensions de l’image fixe"@fr, "dimensions of still image"@en ;
    reg:hasUnconstrained <http://rdaregistry.info/Elements/u/P60541> ;
    reg:lexicalAlias <http://rdaregistry.info/Elements/m/dimensionsOfStillImage.en> ;
    reg:name "dimensionsOfStillImage"@en ;
    reg:status <http://metadataregistry.org/uri/RegStatus/1001> ;
    a rdf:Property ;
    rdfs:domain <http://rdaregistry.info/Elements/c/C10007> ;
    rdfs:isDefinedBy <http://rdaregistry.info/Elements/m/> ;
    rdfs:label "a pour dimensions de l’image fixe"@fr, "har bildytans mått"@sv, "has dimensions of still image"@en ;
    rdfs:subPropertyOf <http://rdaregistry.info/Elements/m/P30169> ;
    skos:definition "Met une manifestation en relation avec les mesures de la partie graphique d’une image fixe."@fr, "Relates a manifestation to a measurement of the pictorial area of a still image."@en .

<http://rdaregistry.info/Elements/m/P30172>
    rdakit:instructionNumber "3.16.2" ;
    rdakit:toolkitDefinition "A method used to encode audio content for playback."@en, "El método utilizado para codificar el contenido sonoro para reproducción (por ej., análogo, digital)."@es, "La méthode utilisée pour encoder un contenu audio pour la lecture (par exemple, analogique, numérique)."@fr ;
    rdakit:toolkitLabel "inspelningstyp"@sv, "tipo de grabación"@es, "type d’enregistrement"@fr, "type of recording"@en ;
    reg:hasUnconstrained <http://rdaregistry.info/Elements/u/P60543> ;
    reg:lexicalAlias <http://rdaregistry.info/Elements/m/typeOfRecording.en> ;
    reg:name "typeOfRecording"@en ;
    reg:status <http://metadataregistry.org/uri/RegStatus/1001> ;
    a rdf:Property ;
    rdfs:domain <http://rdaregistry.info/Elements/c/C10007> ;
    rdfs:isDefinedBy <http://rdaregistry.info/Elements/m/> ;
    rdfs:label "a pour type d’enregistrement"@fr, "har inspelningstyp"@sv, "has type of recording"@en ;
    rdfs:subPropertyOf <http://rdaregistry.info/Elements/m/P30125> ;
    skos:definition "Met une manifestation en relation avec la méthode utilisée pour encoder un contenu audio pour la lecture (par exemple, analogique, numérique)."@fr, "Relates a manifestation to a method used to encode audio content for playback."@en .

<http://rdaregistry.info/Elements/m/P30173>
    rdakit:instructionNumber "2.9.4" ;
    rdakit:toolkitDefinition "A name of an agent responsible for distributing a manifestation in a published form."@en, "El nombre de una persona, familia o entidad corporativa responsable de la distribución de un recurso publicado."@es, "Le nom d’une personne, famille ou collectivité responsable de la diffusion ou de la distribution d’une ressource sous une forme publiée."@fr ;
    rdakit:toolkitLabel "distributor's name"@en, "distributörsnamn"@sv, "nom du diffuseur ou du distributeur"@fr, "nombre del distribuidor"@es ;
    reg:hasUnconstrained <http://rdaregistry.info/Elements/u/P60544> ;
    reg:lexicalAlias <http://rdaregistry.info/Elements/m/distributorsName.en> ;
    reg:name "distributorsName"@en ;
    reg:status <http://metadataregistry.org/uri/RegStatus/1001> ;
    a rdf:Property ;
    rdfs:domain <http://rdaregistry.info/Elements/c/C10007> ;
    rdfs:isDefinedBy <http://rdaregistry.info/Elements/m/> ;
    rdfs:label "a pour nom du diffuseur ou du distributeur"@fr, "har distributörsnamn"@sv, "has distributor’s name"@en ;
    skos:definition "Met une manifestation en relation avec le nom d’une personne, famille ou collectivité responsable de la diffusion ou de la distribution d’une ressource sous une forme publiée."@fr, "Relates a manifestation to a name of an agent responsible for distributing a manifestation in a published form."@en .

<http://rdaregistry.info/Elements/m/P30174>
    rdakit:instructionNumber "2.7.4" ;
    rdakit:toolkitDefinition "A name of an agent responsible for inscribing, fabricating, constructing, etc., a manifestation in an unpublished form."@en, "El nombre de una persona, familia o entidad corporativa responsable de la inscripción, fabricación, construcción, etc., de un recurso en un formato inédito."@es, "Le nom d’une personne, famille ou collectivité responsable de la scription, de la fabrication, de la construction, etc. d’une ressource sous une forme non publiée."@fr ;
    rdakit:toolkitLabel "nom du producteur"@fr, "nombre del productor"@es, "producentnamn"@sv, "producer's name"@en ;
    reg:hasUnconstrained <http://rdaregistry.info/Elements/u/P60545> ;
    reg:lexicalAlias <http://rdaregistry.info/Elements/m/producersName.en> ;
    reg:name "producersName"@en ;
    reg:status <http://metadataregistry.org/uri/RegStatus/1001> ;
    a rdf:Property ;
    rdfs:domain <http://rdaregistry.info/Elements/c/C10007> ;
    rdfs:isDefinedBy <http://rdaregistry.info/Elements/m/> ;
    rdfs:label "a pour nom du producteur"@fr, "har producentnamn"@sv, "has producer’s name"@en ;
    skos:definition "Met une manifestation en relation avec le nom d’une personne, famille ou collectivité responsable de la scription, de la fabrication, de la construction, etc. d’une ressource sous une forme non publiée."@fr, "Relates a manifestation to a name of an agent responsible for inscribing, fabricating, constructing, etc., a manifestation in an unpublished form."@en .

<http://rdaregistry.info/Elements/m/P30175>
    rdakit:instructionNumber "2.10.4" ;
    rdakit:toolkitDefinition "A name of an agent responsible for printing, duplicating, casting, etc., a manifestation in a published form."@en, "El nombre de una persona, familia o entidad corporativa responsable por la impresión, duplicación prensado etc., de un recurso publicado."@es, "Le nom d’une personne, famille ou collectivité responsable de l’impression, de la reproduction, du moulage, etc. d’une ressource sous une forme publiée."@fr ;
    rdakit:toolkitLabel "manufacturer's name"@en, "nom du fabricant"@fr, "nombre del fabricante"@es, "tillverkarnamn"@sv ;
    reg:hasUnconstrained <http://rdaregistry.info/Elements/u/P60546> ;
    reg:lexicalAlias <http://rdaregistry.info/Elements/m/manufacturersName.en> ;
    reg:name "manufacturersName"@en ;
    reg:status <http://metadataregistry.org/uri/RegStatus/1001> ;
    a rdf:Property ;
    rdfs:domain <http://rdaregistry.info/Elements/c/C10007> ;
    rdfs:isDefinedBy <http://rdaregistry.info/Elements/m/> ;
    rdfs:label "a pour nom du fabricant"@fr, "har tillverkarnamn"@sv, "has manufacturer’s name"@en ;
    skos:definition "Met une manifestation en relation avec le nom d’une personne, famille ou collectivité responsable de l’impression, de la reproduction, du moulage, etc. d’une ressource sous une forme publiée."@fr, "Relates a manifestation to a name of an agent responsible for printing, duplicating, casting, etc., a manifestation in a published form."@en .

<http://rdaregistry.info/Elements/m/P30176>
    rdakit:instructionNumber "2.8.4" ;
    rdakit:toolkitDefinition "A name of an agent responsible for publishing, releasing, or issuing a manifestation."@en, "El nombre de una persona, familia o entidad corporativa responsable por la publicación, entrega o emisión de un recurso."@es, "Le nom d’une personne, famille ou collectivité responsable de la publication, de la mise à disposition ou de l’édition d’une ressource."@fr ;
    rdakit:toolkitLabel "nom de l’éditeur"@fr, "nombre del editor"@es, "publisher's name"@en, "utgivarnamn"@sv ;
    reg:hasUnconstrained <http://rdaregistry.info/Elements/u/P60547> ;
    reg:lexicalAlias <http://rdaregistry.info/Elements/m/publishersName.en> ;
    reg:name "publishersName"@en ;
    reg:status <http://metadataregistry.org/uri/RegStatus/1001> ;
    a rdf:Property ;
    rdfs:domain <http://rdaregistry.info/Elements/c/C10007> ;
    rdfs:isDefinedBy <http://rdaregistry.info/Elements/m/> ;
    rdfs:label "a pour nom de l’éditeur"@fr, "har utgivarnamn"@sv, "has publisher’s name"@en ;
    skos:definition "Met une manifestation en relation avec le nom d’une personne, famille ou collectivité responsable de la publication, de la mise à disposition ou de l’édition d’une ressource."@fr, "Relates a manifestation to a name of an agent responsible for publishing, releasing, or issuing a manifestation."@en .

<http://rdaregistry.info/Elements/m/P30177>
    rdakit:toolkitDefinition "El número y tipo de unidades y/o subunidades que constituyen un recurso cartográfico."@es, "Le nombre et le type d’unités et/ou de sous-unités formant une ressource cartographique."@fr ;
    rdakit:toolkitLabel "extensión de recurso cartográfico"@es, "importance matérielle de la ressource cartographique"@fr ;
    reg:hasUnconstrained <http://rdaregistry.info/Elements/u/P60550> ;
    reg:lexicalAlias <http://rdaregistry.info/Elements/m/extentOfCartographicResource.en> ;
    reg:name "extentOfCartographicResource"@en ;
    reg:status <http://metadataregistry.org/uri/RegStatus/1008> ;
    a rdf:Property ;
    rdfs:domain <http://rdaregistry.info/Elements/c/C10007> ;
    rdfs:isDefinedBy <http://rdaregistry.info/Elements/m/> ;
    rdfs:label "a pour importance matérielle de la ressource cartographique"@fr, "has extent of cartographic resource (Deprecated)"@en ;
    rdfs:subPropertyOf <http://rdaregistry.info/Elements/m/P30182> ;
    skos:definition "Met une manifestation en relation avec le nombre et le type d’unités et/ou de sous-unités formant une ressource cartographique."@fr .

<http://rdaregistry.info/Elements/m/P30178>
    rdakit:toolkitDefinition "El número y tipo de unidades y/o subunidades que constituyen un recurso que consiste en música notada (con o sin acompañamiento de texto y/o ilustraciones)."@es, "Le nombre et le type d’unités et/ou de sous-unités formant une ressource constituée de musique notée, avec ou sans texte d’accompagnement et/ou illustrations."@fr ;
    rdakit:toolkitLabel "extensión de la música notada"@es, "importance matérielle de la musique notée"@fr ;
    reg:hasUnconstrained <http://rdaregistry.info/Elements/u/P60550> ;
    reg:lexicalAlias <http://rdaregistry.info/Elements/m/extentOfNotatedMusic.en> ;
    reg:name "extentOfNotatedMusic"@en ;
    reg:status <http://metadataregistry.org/uri/RegStatus/1008> ;
    a rdf:Property ;
    rdfs:domain <http://rdaregistry.info/Elements/c/C10007> ;
    rdfs:isDefinedBy <http://rdaregistry.info/Elements/m/> ;
    rdfs:label "a pour importance matérielle de la musique notée"@fr, "has extent of notated music (Deprecated)"@en ;
    rdfs:subPropertyOf <http://rdaregistry.info/Elements/m/P30182> ;
    skos:definition "Met une manifestation en relation avec le nombre et le type d’unités et/ou de sous-unités formant une ressource constituée de musique notée, avec ou sans texte d’accompagnement et/ou illustrations."@fr .

<http://rdaregistry.info/Elements/m/P30179>
    rdakit:toolkitDefinition "El número y tipo de unidades y/o subunidades que constituyen un recurso que consiste en una o más imágenes fijas."@es, "Le nombre et le type d’unités et/ou de sous-unités formant une ressource constituée d’une ou de plusieurs images fixes."@fr ;
    rdakit:toolkitLabel "extensión de la imagen fija"@es, "importance matérielle de l’image fixe"@fr ;
    reg:hasUnconstrained <http://rdaregistry.info/Elements/u/P60550> ;
    reg:lexicalAlias <http://rdaregistry.info/Elements/m/extentOfStillImage.en> ;
    reg:name "extentOfStillImage"@en ;
    reg:status <http://metadataregistry.org/uri/RegStatus/1008> ;
    a rdf:Property ;
    rdfs:domain <http://rdaregistry.info/Elements/c/C10007> ;
    rdfs:isDefinedBy <http://rdaregistry.info/Elements/m/> ;
    rdfs:label "a pour importance matérielle de l’image fixe"@fr, "has extent of still image (Deprecated)"@en ;
    rdfs:subPropertyOf <http://rdaregistry.info/Elements/m/P30182> ;
    skos:definition "Met une manifestation en relation avec le nombre et le type d’unités et/ou de sous-unités formant une ressource constituée d’une ou de plusieurs images fixes."@fr .

<http://rdaregistry.info/Elements/m/P30180>
    rdakit:toolkitDefinition "El número y tipo de unidades y/o subunidades que constituyen un recurso que consiste en una o más formas tridimensionales."@es, "Le nombre et le type d’unités et/ou de sous-unités formant une ressource constituée d’une ou de plusieurs formes tridimensionnelles."@fr ;
    rdakit:toolkitLabel "extensión de la forma tridimensional"@es, "importance matérielle de la forme tridimensionnelle"@fr ;
    reg:hasUnconstrained <http://rdaregistry.info/Elements/u/P60550> ;
    reg:lexicalAlias <http://rdaregistry.info/Elements/m/extentOfThreeDimensionalForm.en> ;
    reg:name "extentOfThreeDimensionalForm"@en ;
    reg:status <http://metadataregistry.org/uri/RegStatus/1008> ;
    a rdf:Property ;
    rdfs:domain <http://rdaregistry.info/Elements/c/C10007> ;
    rdfs:isDefinedBy <http://rdaregistry.info/Elements/m/> ;
    rdfs:label "a pour importance matérielle de la forme tridimensionnelle"@fr, "has extent of three-dimensional form (Deprecated)"@en ;
    rdfs:subPropertyOf <http://rdaregistry.info/Elements/m/P30182> ;
    skos:definition "Met une manifestation en relation avec le nombre et le type d’unités et/ou de sous-unités formant une ressource constituée d’une ou de plusieurs formes tridimensionnelles."@fr .

<http://rdaregistry.info/Elements/m/P30181>
    rdakit:toolkitDefinition "El número y tipo de unidades y/o subunidades que constituyen un recurso que consiste en texto (con o sin ilustraciones)."@es, "Le nombre et le type d’unités et/ou de sous-unités formant une ressource constituée de texte, avec ou sans illustrations."@fr ;
    rdakit:toolkitLabel "extensión del texto"@es, "importance matérielle du texte"@fr ;
    reg:hasUnconstrained <http://rdaregistry.info/Elements/u/P60550> ;
    reg:lexicalAlias <http://rdaregistry.info/Elements/m/extentOfText.en> ;
    reg:name "extentOfText"@en ;
    reg:status <http://metadataregistry.org/uri/RegStatus/1008> ;
    a rdf:Property ;
    rdfs:domain <http://rdaregistry.info/Elements/c/C10007> ;
    rdfs:isDefinedBy <http://rdaregistry.info/Elements/m/> ;
    rdfs:label "a pour importance matérielle du texte"@fr, "has extent of text (Deprecated)"@en ;
    rdfs:subPropertyOf <http://rdaregistry.info/Elements/m/P30182> ;
    skos:definition "Met une manifestation en relation avec le nombre et le type d’unités et/ou de sous-unités formant une ressource constituée de texte, avec ou sans illustrations."@fr .

<http://rdaregistry.info/Elements/m/P30182>
    rdakit:instructionNumber "3.4" ;
    rdakit:toolkitDefinition "A number and type of unit and/or subunit of a manifestation."@en, "El número y tipo de unidades y/o subunidades que constituyen un recurso."@es, "Le nombre et le type d’unités et/ou de sous-unités formant une ressource."@fr ;
    rdakit:toolkitLabel "extensión"@es, "extent"@en, "importance matérielle"@fr, "omfång"@sv ;
    reg:hasSubproperty <http://rdaregistry.info/Elements/m/P30177>, <http://rdaregistry.info/Elements/m/P30178>, <http://rdaregistry.info/Elements/m/P30179>, <http://rdaregistry.info/Elements/m/P30180>, <http://rdaregistry.info/Elements/m/P30181> ;
    reg:hasUnconstrained <http://rdaregistry.info/Elements/u/P60550> ;
    reg:lexicalAlias <http://rdaregistry.info/Elements/m/extent.en> ;
    reg:name "extent"@en ;
    reg:status <http://metadataregistry.org/uri/RegStatus/1001> ;
    a rdf:Property ;
    rdfs:domain <http://rdaregistry.info/Elements/c/C10007> ;
    rdfs:isDefinedBy <http://rdaregistry.info/Elements/m/> ;
    rdfs:label "a pour importance matérielle"@fr, "har omfång"@sv, "has extent"@en ;
    skos:definition "Met une manifestation en relation avec le nombre et le type d’unités et/ou de sous-unités formant une ressource."@fr, "Relates a manifestation to a number and type of unit or subunit of a manifestation."@en .

<http://rdaregistry.info/Elements/m/P30183>
    rdakit:instructionNumber "3.19.4" ;
    rdakit:toolkitDefinition "A number of bytes in a digital file."@en, "El número de bytes en un archivo digital."@es, "Le nombre d’octets d’un fichier numérique."@fr ;
    rdakit:toolkitLabel "file size"@en, "filstorlek"@sv, "taille du fichier"@fr, "tamaño del archivo"@es ;
    reg:hasUnconstrained <http://rdaregistry.info/Elements/u/P60551> ;
    reg:lexicalAlias <http://rdaregistry.info/Elements/m/fileSize.en> ;
    reg:name "fileSize"@en ;
    reg:status <http://metadataregistry.org/uri/RegStatus/1001> ;
    a rdf:Property ;
    rdfs:domain <http://rdaregistry.info/Elements/c/C10007> ;
    rdfs:isDefinedBy <http://rdaregistry.info/Elements/m/> ;
    rdfs:label "a pour taille du fichier"@fr, "har filstorlek"@sv, "has file size"@en ;
    rdfs:subPropertyOf <http://rdaregistry.info/Elements/m/P30124> ;
    skos:definition "Met une manifestation en relation avec le nombre d’octets d’un fichier numérique."@fr, "Relates a manifestation to a number of bytes in a digital file."@en .

<http://rdaregistry.info/Elements/m/P30184>
    rdakit:instructionNumber "3.16.8" ;
    rdakit:toolkitDefinition "A number of sound channels used to make a recording."@en, "El número de canales sonoros utilizados para hacer una grabación (por ej., un canal para una grabación monofónica, dos canales para una grabación estereofónica)."@es, "Le nombre de canaux sonores utilisés pour réaliser un enregistrement (par exemple, un canal pour un enregistrement monophonique, deux canaux pour un enregistrement stéréophonique)."@fr ;
    rdakit:toolkitLabel "antal ljudkanaler"@sv, "configuración de los canales de reproducción sonora"@es, "configuration des canaux de reproduction"@fr, "configuration of playback channels"@en ;
    reg:hasUnconstrained <http://rdaregistry.info/Elements/u/P60552> ;
    reg:lexicalAlias <http://rdaregistry.info/Elements/m/configurationOfPlaybackChannels.en> ;
    reg:name "configurationOfPlaybackChannels"@en ;
    reg:status <http://metadataregistry.org/uri/RegStatus/1001> ;
    a rdf:Property ;
    rdfs:domain <http://rdaregistry.info/Elements/c/C10007> ;
    rdfs:isDefinedBy <http://rdaregistry.info/Elements/m/> ;
    rdfs:label "a pour configuration des canaux de reproduction"@fr, "har antal ljudkanaler"@sv, "has configuration of playback channels"@en ;
    rdfs:subPropertyOf <http://rdaregistry.info/Elements/m/P30125> ;
    skos:definition "Met une manifestation en relation avec le nombre de canaux sonores utilisés pour réaliser un enregistrement (par exemple, un canal pour un enregistrement monophonique, deux canaux pour un enregistrement stéréophonique)."@fr, "Relates a manifestation to a number of sound channels used to make a recording."@en .

<http://rdaregistry.info/Elements/m/P30185>
    rdakit:instructionNumber "3.16.7" ;
    rdakit:toolkitDefinition "A number of tracks on an audiotape."@en, "El número de pistas en una cinta de audio."@es, "Le nombre de pistes sur une bande audio."@fr ;
    rdakit:toolkitLabel "antal spår"@sv, "configuración de cinta"@es, "configuration de bande magnétique"@fr, "tape configuration"@en ;
    reg:hasUnconstrained <http://rdaregistry.info/Elements/u/P60553> ;
    reg:lexicalAlias <http://rdaregistry.info/Elements/m/tapeConfiguration.en> ;
    reg:name "tapeConfiguration"@en ;
    reg:status <http://metadataregistry.org/uri/RegStatus/1001> ;
    a rdf:Property ;
    rdfs:domain <http://rdaregistry.info/Elements/c/C10007> ;
    rdfs:isDefinedBy <http://rdaregistry.info/Elements/m/> ;
    rdfs:label "a pour configuration de bande magnétique"@fr, "har antal spår"@sv, "has tape configuration"@en ;
    rdfs:subPropertyOf <http://rdaregistry.info/Elements/m/P30125> ;
    skos:definition "Met une manifestation en relation avec le nombre de pistes sur une bande audio."@fr, "Relates a manifestation to a number of tracks on an audiotape."@en .

<http://rdaregistry.info/Elements/m/P30186>
    rdakit:instructionNumber "3.8" ;
    rdakit:toolkitDefinition "A physical material used for the support or backing to which the base material of a manifestation has been attached."@en, "El material físico usado como soporte en el cual se sostiene el material base de un recurso."@es, "Le matériau physique utilisé pour le support ou le renforcement, sur lequel le matériau de base d’une ressource est fixé."@fr ;
    rdakit:toolkitLabel "montering"@sv, "montura"@es, "monture"@fr, "mount"@en ;
    reg:hasUnconstrained <http://rdaregistry.info/Elements/u/P60554> ;
    reg:lexicalAlias <http://rdaregistry.info/Elements/m/mount.en> ;
    reg:name "mount"@en ;
    reg:status <http://metadataregistry.org/uri/RegStatus/1001> ;
    a rdf:Property ;
    rdfs:domain <http://rdaregistry.info/Elements/c/C10007> ;
    rdfs:isDefinedBy <http://rdaregistry.info/Elements/m/> ;
    rdfs:label "a pour monture"@fr, "har montering"@sv, "has mount"@en ;
    skos:definition "Met une manifestation en relation avec le matériau physique utilisé pour le support ou le renforcement, sur lequel le matériau de base d’une ressource est fixé."@fr, "Relates a manifestation to a physical material used for the support or backing to which the base material of a manifestation has been attached."@en .

<http://rdaregistry.info/Elements/m/P30187>
    rdakit:instructionNumber "3.9" ;
    rdakit:toolkitDefinition "A process used to produce a manifestation."@en, "El proceso utilizado para producir un recurso."@es, "Le procédé utilisé pour produire une ressource."@fr ;
    rdakit:toolkitLabel "méthode de production"@fr, "método de producción"@es, "production method"@en, "produktionsmetod"@sv ;
    reg:hasSubproperty <http://rdaregistry.info/Elements/m/P30188>, <http://rdaregistry.info/Elements/m/P30189> ;
    reg:hasUnconstrained <http://rdaregistry.info/Elements/u/P60560> ;
    reg:lexicalAlias <http://rdaregistry.info/Elements/m/productionMethod.en> ;
    reg:name "productionMethod"@en ;
    reg:status <http://metadataregistry.org/uri/RegStatus/1001> ;
    a rdf:Property ;
    rdfs:domain <http://rdaregistry.info/Elements/c/C10007> ;
    rdfs:isDefinedBy <http://rdaregistry.info/Elements/m/> ;
    rdfs:label "a pour méthode de production"@fr, "har produktionsmetod"@sv, "has production method"@en ;
    skos:definition "Met une manifestation en relation avec le procédé utilisé pour produire une ressource."@fr, "Relates a manifestation to a process used to produce a manifestation."@en .

<http://rdaregistry.info/Elements/m/P30188>
    rdakit:toolkitDefinition "El proceso utilizado para producir un recurso táctil (por ej., repujado, termoformado)."@es, "Le procédé utilisé pour produire une ressource tactile (par exemple, embossage, thermoformage)."@fr ;
    rdakit:toolkitLabel "méthode de production d’une ressource tactile"@fr, "método de producción de un recurso táctil"@es, "production method for tactile resource"@en ;
    reg:hasUnconstrained <http://rdaregistry.info/Elements/u/P60561> ;
    reg:lexicalAlias <http://rdaregistry.info/Elements/m/productionMethodForTactileResource.en> ;
    reg:name "productionMethodForTactileResource"@en ;
    reg:status <http://metadataregistry.org/uri/RegStatus/1008> ;
    a rdf:Property ;
    rdfs:domain <http://rdaregistry.info/Elements/c/C10007> ;
    rdfs:isDefinedBy <http://rdaregistry.info/Elements/m/> ;
    rdfs:label "a pour méthode de production d’une ressource tactile"@fr ;
    rdfs:subPropertyOf <http://rdaregistry.info/Elements/m/P30187> ;
    skos:definition "Met une manifestation en relation avec le procédé utilisé pour produire une ressource tactile (par exemple, embossage, thermoformage)."@fr .

<http://rdaregistry.info/Elements/m/P30189>
    rdakit:toolkitDefinition "El proceso utilizado para producir un manuscrito original o una copia."@es, "Le procédé utilisé pour produire un manuscrit original ou une copie."@fr, "The process used to produce an original manuscript or a copy."@en ;
    rdakit:toolkitLabel "méthode de production d’un manuscrit"@fr, "método de producción para un manuscrito"@es, "production method for manuscript"@en ;
    reg:hasUnconstrained <http://rdaregistry.info/Elements/u/P60562> ;
    reg:lexicalAlias <http://rdaregistry.info/Elements/m/productionMethodForManuscript.en> ;
    reg:name "productionMethodForManuscript"@en ;
    reg:status <http://metadataregistry.org/uri/RegStatus/1008> ;
    a rdf:Property ;
    rdfs:domain <http://rdaregistry.info/Elements/c/C10007> ;
    rdfs:isDefinedBy <http://rdaregistry.info/Elements/m/> ;
    rdfs:label "a pour méthode de production d’un manuscrit"@fr ;
    rdfs:subPropertyOf <http://rdaregistry.info/Elements/m/P30187> ;
    skos:definition "Met une manifestation en relation avec le procédé utilisé pour produire un manuscrit original ou une copie."@fr, "Relates a manifestation to the process used to produce an original manuscript or a copy."@en .

<http://rdaregistry.info/Elements/m/P30190>
    rdakit:toolkitDefinition "La relación entre un soporte de audio original y el soporte de una reproducción hecha del original (por ej., cinta maestra de duplicación, una impresión de prueba)."@es, "La relation entre un support matériel original d’un enregistrement audio et le support matériel d’une reproduction faite à partir de l’original (par exemple, une matrice de duplication de bande, un disque-épreuve)."@fr ;
    rdakit:toolkitLabel "generación de la grabación sonora"@es, "generation of audio recording"@en, "génération d’enregistrement audio"@fr ;
    reg:hasUnconstrained <http://rdaregistry.info/Elements/u/P60567> ;
    reg:lexicalAlias <http://rdaregistry.info/Elements/m/generationOfAudioRecording.en> ;
    reg:name "generationOfAudioRecording"@en ;
    reg:status <http://metadataregistry.org/uri/RegStatus/1008> ;
    a rdf:Property ;
    rdfs:domain <http://rdaregistry.info/Elements/c/C10007> ;
    rdfs:isDefinedBy <http://rdaregistry.info/Elements/m/> ;
    rdfs:label "a pour génération d’enregistrement audio"@fr ;
    rdfs:subPropertyOf <http://rdaregistry.info/Elements/m/P30191> ;
    skos:definition "Met une manifestation en relation avec la relation entre un support matériel original d’un enregistrement audio et le support matériel d’une reproduction faite à partir de l’original (par exemple, une matrice de duplication de bande, un disque-épreuve)."@fr .

<http://rdaregistry.info/Elements/m/P30191>
    rdakit:instructionNumber "3.10" ;
    rdakit:toolkitDefinition "A relationship between an original carrier and the carrier of a reproduction made from the original."@en, "La relación entre un soporte original y el soporte de una reproducción del original (por ej., una cámara maestra de primera generación, una impresión maestra de segunda generación)."@es, "La relation entre un support matériel original et le support matériel d’une reproduction faite à partir de l’original (par exemple, un microfilm de prise de vue (première génération), une matrice (deuxième génération))."@fr ;
    rdakit:toolkitLabel "generación"@es, "generation"@en, "generation"@sv, "génération"@fr ;
    reg:hasSubproperty <http://rdaregistry.info/Elements/m/P30190>, <http://rdaregistry.info/Elements/m/P30192>, <http://rdaregistry.info/Elements/m/P30193>, <http://rdaregistry.info/Elements/m/P30194>, <http://rdaregistry.info/Elements/m/P30195> ;
    reg:hasUnconstrained <http://rdaregistry.info/Elements/u/P60568> ;
    reg:lexicalAlias <http://rdaregistry.info/Elements/m/generation.en> ;
    reg:name "generation"@en ;
    reg:status <http://metadataregistry.org/uri/RegStatus/1001> ;
    a rdf:Property ;
    rdfs:domain <http://rdaregistry.info/Elements/c/C10007> ;
    rdfs:isDefinedBy <http://rdaregistry.info/Elements/m/> ;
    rdfs:label "a pour génération"@fr, "har generation"@sv, "has generation"@en ;
    skos:definition "Met une manifestation en relation avec la relation entre un support matériel original et le support matériel d’une reproduction faite à partir de l’original (par exemple, un microfilm de prise de vue (première génération), une matrice (deuxième génération))."@fr, "Relates a manifestation to a relationship between an original carrier and the carrier of a reproduction made from the original."@en .

<http://rdaregistry.info/Elements/m/P30192>
    rdakit:toolkitDefinition "La relación entre el soporte original de un recurso digital y el soporte de una reproducción del original (por ej., máster derivado)."@es, "La relation entre un support matériel original d’une ressource numérique et le support matériel d’une reproduction faite à partir de l’original (par exemple, une matrice de dérivation)."@fr ;
    rdakit:toolkitLabel "generación del recurso digital"@es, "generation of digital resource"@en, "génération de ressource numérique"@fr ;
    reg:hasUnconstrained <http://rdaregistry.info/Elements/u/P60569> ;
    reg:lexicalAlias <http://rdaregistry.info/Elements/m/generationOfDigitalResource.en> ;
    reg:name "generationOfDigitalResource"@en ;
    reg:status <http://metadataregistry.org/uri/RegStatus/1008> ;
    a rdf:Property ;
    rdfs:domain <http://rdaregistry.info/Elements/c/C10007> ;
    rdfs:isDefinedBy <http://rdaregistry.info/Elements/m/> ;
    rdfs:label "a pour génération de ressource numérique"@fr ;
    rdfs:subPropertyOf <http://rdaregistry.info/Elements/m/P30191> ;
    skos:definition "Met une manifestation en relation avec la relation entre un support matériel original d’une ressource numérique et le support matériel d’une reproduction faite à partir de l’original (par exemple, une matrice de dérivation)."@fr .

<http://rdaregistry.info/Elements/m/P30193>
    rdakit:toolkitDefinition "La relación entre un soporte original de una película cinematográfica como recurso y el soporte de la reproducción hecha del original (por ej., impreso de referencia)."@es, "La relation entre un support matériel original d’une ressource filmique et le support matériel d’une reproduction faite à partir de l’original (par exemple, une copie de référence)."@fr ;
    rdakit:toolkitLabel "generación de la película cinematográfica"@es, "generation of motion picture film"@en, "génération de film cinématographique"@fr ;
    reg:hasUnconstrained <http://rdaregistry.info/Elements/u/P60570> ;
    reg:lexicalAlias <http://rdaregistry.info/Elements/m/generationOfMotionPictureFilm.en> ;
    reg:name "generationOfMotionPictureFilm"@en ;
    reg:status <http://metadataregistry.org/uri/RegStatus/1008> ;
    a rdf:Property ;
    rdfs:domain <http://rdaregistry.info/Elements/c/C10007> ;
    rdfs:isDefinedBy <http://rdaregistry.info/Elements/m/> ;
    rdfs:label "a pour génération de film cinématographique"@fr ;
    rdfs:subPropertyOf <http://rdaregistry.info/Elements/m/P30191> ;
    skos:definition "Met une manifestation en relation avec la relation entre un support matériel original d’une ressource filmique et le support matériel d’une reproduction faite à partir de l’original (par exemple, une copie de référence)."@fr .

<http://rdaregistry.info/Elements/m/P30194>
    rdakit:toolkitDefinition "La relación entre un soporte original de un recurso en videocinta y el soporte de una reproducción hecha del original (por ej., copia de exhibición)."@es, "La relation entre un support matériel original d’une ressource sur bande vidéo et le support matériel d’une reproduction faite à partir de l’original (par exemple, une copie de présentation)."@fr ;
    rdakit:toolkitLabel "generación de la videocinta"@es, "generation of videotape"@en, "génération de bande vidéo"@fr ;
    reg:hasUnconstrained <http://rdaregistry.info/Elements/u/P60571> ;
    reg:lexicalAlias <http://rdaregistry.info/Elements/m/generationOfVideotape.en> ;
    reg:name "generationOfVideotape"@en ;
    reg:status <http://metadataregistry.org/uri/RegStatus/1008> ;
    a rdf:Property ;
    rdfs:domain <http://rdaregistry.info/Elements/c/C10007> ;
    rdfs:isDefinedBy <http://rdaregistry.info/Elements/m/> ;
    rdfs:label "a pour génération de bande vidéo"@fr ;
    rdfs:subPropertyOf <http://rdaregistry.info/Elements/m/P30191> ;
    skos:definition "Met une manifestation en relation avec la relation entre un support matériel original d’une ressource sur bande vidéo et le support matériel d’une reproduction faite à partir de l’original (par exemple, une copie de présentation)."@fr .

<http://rdaregistry.info/Elements/m/P30195>
    rdakit:toolkitDefinition "La relación entre el soporte original de una microforma y el soporte de una reproducción hecha del original (por ej., un máster de impresión)."@es, "La relation entre un support matériel original d’une ressource sur microforme et le support matériel d’une reproduction faite à partir de l’original (par exemple, matrice)."@fr ;
    rdakit:toolkitLabel "generación de la microforma"@es, "generation of microform"@en, "génération de microforme"@fr ;
    reg:hasUnconstrained <http://rdaregistry.info/Elements/u/P60572> ;
    reg:lexicalAlias <http://rdaregistry.info/Elements/m/generationOfMicroform.en> ;
    reg:name "generationOfMicroform"@en ;
    reg:status <http://metadataregistry.org/uri/RegStatus/1008> ;
    a rdf:Property ;
    rdfs:domain <http://rdaregistry.info/Elements/c/C10007> ;
    rdfs:isDefinedBy <http://rdaregistry.info/Elements/m/> ;
    rdfs:label "a pour génération de microforme"@fr ;
    rdfs:subPropertyOf <http://rdaregistry.info/Elements/m/P30191> ;
    skos:definition "Met une manifestation en relation avec la relation entre un support matériel original d’une ressource sur microforme et le support matériel d’une reproduction faite à partir de l’original (par exemple, matrice)."@fr .

<http://rdaregistry.info/Elements/m/P30196>
    rdakit:instructionNumber "3.14" ;
    rdakit:toolkitDefinition "A relationship of the colours and tones in an image to the colours and tones of the object reproduced."@en, "La relación de los colores y tonos en una imagen con los colores y tonos del objeto reproducido (por ej., positiva, negativa)."@es, "La relation des couleurs et des tons d’une image avec les couleurs et les tons de l’objet reproduit (par exemple, positif, négatif)."@fr ;
    rdakit:toolkitLabel "polaridad"@es, "polaritet"@sv, "polarity"@en, "polarité"@fr ;
    reg:hasUnconstrained <http://rdaregistry.info/Elements/u/P60573> ;
    reg:lexicalAlias <http://rdaregistry.info/Elements/m/polarity.en> ;
    reg:name "polarity"@en ;
    reg:status <http://metadataregistry.org/uri/RegStatus/1001> ;
    a rdf:Property ;
    rdfs:domain <http://rdaregistry.info/Elements/c/C10007> ;
    rdfs:isDefinedBy <http://rdaregistry.info/Elements/m/> ;
    rdfs:label "a pour polarité"@fr, "har polaritet"@sv, "has polarity"@en ;
    skos:definition "Met une manifestation en relation avec la relation des couleurs et des tons d’une image avec les couleurs et les tons de l’objet reproduit (par exemple, positif, négatif)."@fr, "Relates a manifestation to a relationship of the colours and tones in an image to the colours and tones of the object reproduced."@en .

<http://rdaregistry.info/Elements/m/P30197>
    rdakit:instructionNumber "3.12" ;
    rdakit:toolkitDefinition "A proportional relationship between a whole sheet in a printed or manuscript resource, and the individual leaves that result if that sheet is left full, cut, or folded."@en, "El resultado del plegado de una hoja impresa para formar un conjunto de hojas (por ej., una hoja doblada una vez para formar un folio, dos veces para formar un cuarto, tres veces para formar un octavo)."@es, "Le résultat du pliage d’une feuille imprimée pour former un cahier de feuillets (par exemple, une feuille pliée une fois pour former un in-folio, pliée deux fois pour former un in-quarto, pliée trois fois pour former un in-octavo, etc.)."@fr ;
    rdakit:toolkitLabel "bibliographic format"@en, "bokformat"@sv, "format du livre"@fr, "formato libro"@es ;
    reg:hasUnconstrained <http://rdaregistry.info/Elements/u/P60578> ;
    reg:lexicalAlias <http://rdaregistry.info/Elements/m/bibliographicFormat.en> ;
    reg:name "bibliographicFormat"@en ;
    reg:status <http://metadataregistry.org/uri/RegStatus/1001> ;
    a rdf:Property ;
    rdfs:domain <http://rdaregistry.info/Elements/c/C10007> ;
    rdfs:isDefinedBy <http://rdaregistry.info/Elements/m/> ;
    rdfs:label "a pour format du livre"@fr, "har bokformat"@sv, "has bibliographic format"@en ;
    skos:definition "Met une manifestation en relation avec le résultat du pliage d’une feuille imprimée pour former un cahier de feuillets (par exemple, une feuille pliée une fois pour former un in-folio, pliée deux fois pour former un in-quarto, pliée trois fois pour former un in-octavo, etc.)."@fr, "Relates a manifestation to a proportional relationship between a whole sheet in a printed or manuscript resource, and the individual leaves that result if that sheet is left full, cut, or folded."@en .

<http://rdaregistry.info/Elements/m/P30198>
    rdakit:instructionNumber "3.15" ;
    rdakit:toolkitDefinition "A numerical ratio of the size of a micro-image in relation to the original from which it was produced."@en, "El tamaño de una microimagen en relación con el original del cual se produjo."@es, "La taille d’une micro-image par rapport à celle de l’original à partir duquel elle a été produite."@fr ;
    rdakit:toolkitLabel "escala de reducción"@es, "facteur de réduction"@fr, "förminskningsgrad"@sv, "reduction ratio"@en ;
    reg:hasUnconstrained <http://rdaregistry.info/Elements/u/P60581> ;
    reg:lexicalAlias <http://rdaregistry.info/Elements/m/reductionRatio.en> ;
    reg:name "reductionRatio"@en ;
    reg:status <http://metadataregistry.org/uri/RegStatus/1001> ;
    a rdf:Property ;
    rdfs:domain <http://rdaregistry.info/Elements/c/C10007> ;
    rdfs:isDefinedBy <http://rdaregistry.info/Elements/m/> ;
    rdfs:label "a pour facteur de réduction"@fr, "har förminskningsgrad"@sv, "has reduction ratio"@en ;
    skos:definition "Met une manifestation en relation avec la taille d’une micro-image par rapport à celle de l’original à partir duquel elle a été produite."@fr, "Relates a manifestation to a numerical ratio of the size of a micro-image in relation to the original from which it was produced."@en .

<http://rdaregistry.info/Elements/m/P30199>
    rdakit:instructionNumber "3.13" ;
    rdakit:toolkitDefinition "A size of the type used to represent the characters and symbols in a manifestation."@en, "El tamaño del tipo utilizado para representar los caracteres y símbolos en un recurso."@es, "La taille des caractères utilisés pour représenter les signes et les symboles dans une ressource."@fr ;
    rdakit:toolkitLabel "font size"@en, "taille de la police de caractères"@fr, "tamaño de la fuente"@es, "teckenstorlek"@sv ;
    reg:hasUnconstrained <http://rdaregistry.info/Elements/u/P60582> ;
    reg:lexicalAlias <http://rdaregistry.info/Elements/m/fontSize.en> ;
    reg:name "fontSize"@en ;
    reg:status <http://metadataregistry.org/uri/RegStatus/1001> ;
    a rdf:Property ;
    rdfs:domain <http://rdaregistry.info/Elements/c/C10007> ;
    rdfs:isDefinedBy <http://rdaregistry.info/Elements/m/> ;
    rdfs:label "a pour taille de la police de caractères"@fr, "har teckenstorlek"@sv, "has font size"@en ;
    skos:definition "Met une manifestation en relation avec la taille des caractères utilisés pour représenter les signes et les symboles dans une ressource."@fr, "Relates a manifestation to a size of the type used to represent the characters and symbols in a manifestation."@en .

<http://rdaregistry.info/Elements/m/P30200>
    rdakit:instructionNumber "3.17.3" ;
    rdakit:toolkitDefinition "A speed at which a projected carrier must be operated to produce the moving image intended."@en, "La velocidad a la cual un proyector debe ser operado para producir la imagen en movimiento esperada."@es, "La vitesse à laquelle doit être actionné un support matériel projeté afin de produire l’image animée prévue."@fr ;
    rdakit:toolkitLabel "projection speed"@en, "projektionshastighet"@sv, "velocidad de proyección"@es, "vitesse de projection"@fr ;
    reg:hasUnconstrained <http://rdaregistry.info/Elements/u/P60585> ;
    reg:lexicalAlias <http://rdaregistry.info/Elements/m/projectionSpeed.en> ;
    reg:name "projectionSpeed"@en ;
    reg:status <http://metadataregistry.org/uri/RegStatus/1001> ;
    a rdf:Property ;
    rdfs:domain <http://rdaregistry.info/Elements/c/C10007> ;
    rdfs:isDefinedBy <http://rdaregistry.info/Elements/m/> ;
    rdfs:label "a pour vitesse de projection"@fr, "har projektionshastighet"@sv, "has projection speed"@en ;
    rdfs:subPropertyOf <http://rdaregistry.info/Elements/m/P30127> ;
    skos:definition "Met une manifestation en relation avec la vitesse à laquelle doit être actionné un support matériel projeté afin de produire l’image animée prévue."@fr, "Relates a manifestation to a speed at which a projected carrier must be operated to produce the moving image intended."@en .

<http://rdaregistry.info/Elements/m/P30201>
    rdakit:instructionNumber "3.16.4" ;
    rdakit:toolkitDefinition "A speed at which an audio carrier must be operated to produce the sound intended."@en, "La velocidad a la cual un soporte de audio debe ser operado para producir el sonido esperado."@es, "La vitesse à laquelle un support matériel audio doit être utilisé pour produire le son prévu."@fr ;
    rdakit:toolkitLabel "playing speed"@en, "uppspelningshastighet"@sv, "velocidad de reproducción"@es, "vitesse de lecture"@fr ;
    reg:hasUnconstrained <http://rdaregistry.info/Elements/u/P60586> ;
    reg:lexicalAlias <http://rdaregistry.info/Elements/m/playingSpeed.en> ;
    reg:name "playingSpeed"@en ;
    reg:status <http://metadataregistry.org/uri/RegStatus/1001> ;
    a rdf:Property ;
    rdfs:domain <http://rdaregistry.info/Elements/c/C10007> ;
    rdfs:isDefinedBy <http://rdaregistry.info/Elements/m/> ;
    rdfs:label "a pour vitesse de lecture"@fr, "har uppspelningshastighet"@sv, "has playing speed"@en ;
    rdfs:subPropertyOf <http://rdaregistry.info/Elements/m/P30125> ;
    skos:definition "Met une manifestation en relation avec la vitesse à laquelle un support matériel audio doit être utilisé pour produire le son prévu."@fr, "Relates a manifestation to a speed at which an audio carrier must be operated to produce the sound intended."@en .

<http://rdaregistry.info/Elements/m/P30202>
    rdakit:instructionNumber "3.19.7" ;
    rdakit:toolkitDefinition "A speed at which streaming audio, video, etc., is designed to play."@en, "La velocidad a la que el streaming de audio, video, etc., está diseñado para funcionar."@es, "La vitesse à laquelle un flux audio, vidéo, etc. est destiné à être diffusé."@fr ;
    rdakit:toolkitLabel "bithastighet"@sv, "débit binaire codé"@fr, "encoded bitrate"@en, "velocidad de transmisión codificada"@es ;
    reg:hasUnconstrained <http://rdaregistry.info/Elements/u/P60587> ;
    reg:lexicalAlias <http://rdaregistry.info/Elements/m/encodedBitrate.en> ;
    reg:name "encodedBitrate"@en ;
    reg:status <http://metadataregistry.org/uri/RegStatus/1001> ;
    a rdf:Property ;
    rdfs:domain <http://rdaregistry.info/Elements/c/C10007> ;
    rdfs:isDefinedBy <http://rdaregistry.info/Elements/m/> ;
    rdfs:label "a pour débit binaire codé"@fr, "har bithastighet"@sv, "has encoded bitrate"@en ;
    rdfs:subPropertyOf <http://rdaregistry.info/Elements/m/P30124> ;
    skos:definition "Met une manifestation en relation avec la vitesse à laquelle un flux audio, vidéo, etc. est destiné à être diffusé."@fr, "Relates a manifestation to a speed at which streaming audio, video, etc., is designed to play."@en .

<http://rdaregistry.info/Elements/m/P30203>
    rdakit:instructionNumber "2.3.3" ;
    rdakit:toolkitDefinition "A title proper in another language or script."@en, "El título propiamente dicho en otra lengua y/o escritura."@es, "Le titre propre dans une autre langue et/ou écriture."@fr ;
    rdakit:toolkitLabel "parallel title proper"@en, "parallell huvudtitel"@sv, "titre propre parallèle"@fr, "título paralelo propiamente dicho"@es ;
    reg:hasUnconstrained <http://rdaregistry.info/Elements/u/P60589> ;
    reg:lexicalAlias <http://rdaregistry.info/Elements/m/parallelTitleProper.en> ;
    reg:name "parallelTitleProper"@en ;
    reg:status <http://metadataregistry.org/uri/RegStatus/1001> ;
    a rdf:Property ;
    rdfs:domain <http://rdaregistry.info/Elements/c/C10007> ;
    rdfs:isDefinedBy <http://rdaregistry.info/Elements/m/> ;
    rdfs:label "a pour titre propre parallèle"@fr, "har parallell huvudtitel"@sv, "has parallel title proper"@en ;
    rdfs:subPropertyOf <http://rdaregistry.info/Elements/m/P30134> ;
    skos:definition "Met une manifestation en relation avec le titre propre dans une autre langue et/ou écriture."@fr, "Relates a manifestation to a title proper in another language or script."@en ;
    skos:scopeNote "An alternative title in another language or script is treated as part of a parallel title proper."@en .

<http://rdaregistry.info/Elements/m/P30204>
    rdakit:instructionNumber "2.12.3" ;
    rdakit:toolkitDefinition "A title proper of a series in another language or script."@en, "El título propiamente dicho de una serie en otra lengua y/o escritura."@es, "Le titre propre d’une collection dans une autre langue et/ou écriture."@fr ;
    rdakit:toolkitLabel "parallel title proper of series"@en, "parallell huvudtitel till serie"@sv, "titre propre parallèle de la collection"@fr, "título paralelo propiamente dicho de la serie"@es ;
    reg:hasUnconstrained <http://rdaregistry.info/Elements/u/P60590> ;
    reg:lexicalAlias <http://rdaregistry.info/Elements/m/parallelTitleProperOfSeries.en> ;
    reg:name "parallelTitleProperOfSeries"@en ;
    reg:status <http://metadataregistry.org/uri/RegStatus/1001> ;
    a rdf:Property ;
    rdfs:domain <http://rdaregistry.info/Elements/c/C10007> ;
    rdfs:isDefinedBy <http://rdaregistry.info/Elements/m/> ;
    rdfs:label "a pour titre propre parallèle de la collection"@fr, "har parallel title proper of series"@sv, "has parallel title proper of series"@en ;
    skos:definition "Met une manifestation en relation avec le titre propre d’une collection dans une autre langue et/ou écriture."@fr, "Relates a manifestation to a title proper of a series in another language or script."@en .

<http://rdaregistry.info/Elements/m/P30205>
    rdakit:instructionNumber "2.12.11" ;
    rdakit:toolkitDefinition "A title proper of a subseries in another language or script."@en, "El título propiamente dicho de una subserie en otra lengua y/o escritura."@es, "Le titre propre d’une sous-collection dans une autre langue et/ou écriture."@fr ;
    rdakit:toolkitLabel "parallel title proper of subseries"@en, "parallell huvudtitel till underserie"@sv, "titre propre parallèle de la sous-collection"@fr, "título paralelo propiamente dicho de la subserie"@es ;
    reg:hasUnconstrained <http://rdaregistry.info/Elements/u/P60591> ;
    reg:lexicalAlias <http://rdaregistry.info/Elements/m/parallelTitleProperOfSubseries.en> ;
    reg:name "parallelTitleProperOfSubseries"@en ;
    reg:status <http://metadataregistry.org/uri/RegStatus/1001> ;
    a rdf:Property ;
    rdfs:domain <http://rdaregistry.info/Elements/c/C10007> ;
    rdfs:isDefinedBy <http://rdaregistry.info/Elements/m/> ;
    rdfs:label "a pour titre propre parallèle de la sous-collection"@fr, "har parallell huvudtitel till underserie"@sv, "has parallel title proper of subseries"@en ;
    skos:definition "Met une manifestation en relation avec le titre propre d’une sous-collection dans une autre langue et/ou écriture."@fr, "Relates a manifestation to a title proper of a subseries in another language or script."@en .

<http://rdaregistry.info/Elements/m/P30206>
    rdakit:instructionNumber "3.16.3" ;
    rdakit:toolkitDefinition "A type of medium used to record sound on an audio carrier."@en, "El tipo de medio utilizado para grabar el sonido en un soporte de audio (por ej., magnético, óptico)."@es, "Le type de support utilisé pour enregistrer du son sur un support matériel audio (par exemple, magnétique, optique)."@fr ;
    rdakit:toolkitLabel "inspelningssätt"@sv, "medio de grabación"@es, "recording medium"@en, "support d’enregistrement"@fr ;
    reg:hasUnconstrained <http://rdaregistry.info/Elements/u/P60594> ;
    reg:lexicalAlias <http://rdaregistry.info/Elements/m/recordingMedium.en> ;
    reg:name "recordingMedium"@en ;
    reg:status <http://metadataregistry.org/uri/RegStatus/1001> ;
    a rdf:Property ;
    rdfs:domain <http://rdaregistry.info/Elements/c/C10007> ;
    rdfs:isDefinedBy <http://rdaregistry.info/Elements/m/> ;
    rdfs:label "a pour support d’enregistrement"@fr, "har inspelningssätt"@sv, "has recording medium"@en ;
    rdfs:subPropertyOf <http://rdaregistry.info/Elements/m/P30125> ;
    skos:definition "Met une manifestation en relation avec le type de support utilisé pour enregistrer du son sur un support matériel audio (par exemple, magnétique, optique)."@fr, "Relates a manifestation to a type of medium used to record sound on an audio carrier."@en .

<http://rdaregistry.info/Elements/m/P30207>
    reg:status <http://metadataregistry.org/uri/RegStatus/1008> ;
    a rdf:Property ;
    rdfs:isDefinedBy <http://rdaregistry.info/Elements/m/> .

<http://rdaregistry.info/Elements/m/P30208>
    rdakit:instructionNumber "3.6" ;
    rdakit:toolkitDefinition "An underlying physical material of a manifestation."@en, "Le matériau physique sous-jacent d’une ressource."@fr, "Material físico que sostiene el recurso."@es ;
    rdakit:toolkitLabel "base material"@en, "bärande material"@sv, "material base"@es, "matériau de base"@fr ;
    reg:hasUnconstrained <http://rdaregistry.info/Elements/u/P60596> ;
    reg:lexicalAlias <http://rdaregistry.info/Elements/m/baseMaterial.en> ;
    reg:name "baseMaterial"@en ;
    reg:status <http://metadataregistry.org/uri/RegStatus/1001> ;
    a rdf:Property ;
    rdfs:domain <http://rdaregistry.info/Elements/c/C10007> ;
    rdfs:isDefinedBy <http://rdaregistry.info/Elements/m/> ;
    rdfs:label "a pour matériau de base"@fr, "har bärande material"@sv, "has base material"@en ;
    skos:definition "Met une manifestation en relation avec le matériau physique sous-jacent d’une ressource."@fr, "Relates a manifestation to an underlying physical material of a manifestation."@en .

<http://rdaregistry.info/Elements/m/P30209>
    rdakit:instructionNumber "2.3.9" ;
    rdakit:toolkitDefinition "A unique name assigned to a manifestation by an ISSN registration agency."@en, "El nombre único asignado a un recurso por una agencia de registro del ISSN."@es, "Le nom unique attribué à une ressource par une agence d’enregistrement de l’ISSN."@fr ;
    rdakit:toolkitLabel "key title"@en, "nyckeltitel"@sv, "titre-clé"@fr, "título clave"@es ;
    reg:hasUnconstrained <http://rdaregistry.info/Elements/u/P60597> ;
    reg:lexicalAlias <http://rdaregistry.info/Elements/m/keyTitle.en> ;
    reg:name "keyTitle"@en ;
    reg:status <http://metadataregistry.org/uri/RegStatus/1001> ;
    a rdf:Property ;
    rdfs:domain <http://rdaregistry.info/Elements/c/C10007> ;
    rdfs:isDefinedBy <http://rdaregistry.info/Elements/m/> ;
    rdfs:label "a pour titre-clé"@fr, "har nyckeltitel"@sv, "has key title"@en ;
    rdfs:subPropertyOf <http://rdaregistry.info/Elements/m/P30134> ;
    skos:definition "Met une manifestation en relation avec le nom unique attribué à une ressource par une agence d’enregistrement de l’ISSN."@fr, "Relates a manifestation to a unique name assigned to a manifestation by an ISSN registration agency."@en .

<http://rdaregistry.info/Elements/m/P30210>
    rdakit:instructionNumber "24.5" ;
    rdakit:toolkitDefinition "A manifestation that accompanies or is accompanied by another manifestation."@en, "Manifestation qui accompagne la manifestation ou est accompagnée par elle."@fr, "Una manifestación que acompaña o está acompañado por la manifestación."@es ;
    rdakit:toolkitLabel "accompanying manifestation relationship"@en, "relaciones de manifestación acompañante"@es, "relation de manifestation d’accompagnement"@fr ;
    reg:hasSubproperty <http://rdaregistry.info/Elements/m/P30027>, <http://rdaregistry.info/Elements/m/object/P30210> ;
    reg:hasUnconstrained <http://rdaregistry.info/Elements/u/P60709> ;
    reg:lexicalAlias <http://rdaregistry.info/Elements/m/accompanyingManifestationRelationship.en> ;
    reg:name "accompanyingManifestationRelationship"@en ;
    reg:status <http://metadataregistry.org/uri/RegStatus/1001> ;
    a rdf:Property ;
    rdfs:domain <http://rdaregistry.info/Elements/c/C10007> ;
    rdfs:isDefinedBy <http://rdaregistry.info/Elements/m/> ;
    rdfs:label "a pour relation de manifestation d’accompagnement"@fr, "has accompanying manifestation relationship with"@en ;
    rdfs:subPropertyOf <http://rdaregistry.info/Elements/m/P30048> ;
    skos:definition "Met une manifestation en relation avec une manifestation qui accompagne la manifestation ou est accompagnée par elle."@fr, "Relates a manifestation to a manifestation that accompanies or is accompanied by another manifestation."@en .

<http://rdaregistry.info/Elements/m/P30211>
    reg:status <http://metadataregistry.org/uri/RegStatus/1008> ;
    a rdf:Property ;
    rdfs:isDefinedBy <http://rdaregistry.info/Elements/m/> .

<http://rdaregistry.info/Elements/m/P30212>
    rdakit:instructionNumber "24.5" ;
    rdakit:toolkitDefinition "A manifestation that is equivalent to another manifestation."@en, "Manifestation qui est équivalente à la manifestation."@fr, "Una manifestación que es equivalente a la manifestación."@es ;
    rdakit:toolkitLabel "equivalent manifestation relationship"@en, "relaciones de manifestación equivalente"@es, "relation de manifestation équivalente"@fr ;
    reg:hasSubproperty <http://rdaregistry.info/Elements/m/P30024>, <http://rdaregistry.info/Elements/m/object/P30212> ;
    reg:hasUnconstrained <http://rdaregistry.info/Elements/u/P60712> ;
    reg:lexicalAlias <http://rdaregistry.info/Elements/m/equivalentManifestationRelationship.en> ;
    reg:name "equivalentManifestationRelationship"@en ;
    reg:status <http://metadataregistry.org/uri/RegStatus/1001> ;
    a rdf:Property ;
    rdfs:domain <http://rdaregistry.info/Elements/c/C10007> ;
    rdfs:isDefinedBy <http://rdaregistry.info/Elements/m/> ;
    rdfs:label "a pour relation de manifestation équivalente"@fr, "has equivalent manifestation relationship with"@en ;
    rdfs:subPropertyOf <http://rdaregistry.info/Elements/m/P30048> ;
    skos:definition "Met une manifestation en relation avec une manifestation qui est équivalente à la manifestation."@fr, "Relates a manifestation to a manifestation that is equivalent to another manifestation."@en .

<http://rdaregistry.info/Elements/m/P30213>
    rdakit:instructionNumber "24.5" ;
    rdakit:toolkitDefinition "A manifestation that is contained in or contains another manifestation."@en, "Manifestation qui est contenue dans la manifestation ou la contient."@fr, "Una manifestación que está incluida en, o contiene la manifestación."@es ;
    rdakit:toolkitLabel "relación de la manifestación todo-parte"@es, "relation de manifestation tout-partie"@fr, "whole-part manifestation relationship"@en ;
    reg:hasSubproperty <http://rdaregistry.info/Elements/m/P30020>, <http://rdaregistry.info/Elements/m/P30033>, <http://rdaregistry.info/Elements/m/object/P30213> ;
    reg:hasUnconstrained <http://rdaregistry.info/Elements/u/P60714> ;
    reg:lexicalAlias <http://rdaregistry.info/Elements/m/wholePartManifestationRelationship.en> ;
    reg:name "wholePartManifestationRelationship"@en ;
    reg:status <http://metadataregistry.org/uri/RegStatus/1001> ;
    a rdf:Property ;
    rdfs:domain <http://rdaregistry.info/Elements/c/C10007> ;
    rdfs:isDefinedBy <http://rdaregistry.info/Elements/m/> ;
    rdfs:label "a pour relation de manifestation tout-partie"@fr, "has whole-part manifestation relationship with"@en ;
    rdfs:subPropertyOf <http://rdaregistry.info/Elements/m/P30048> ;
    skos:definition "Met une manifestation en relation avec une manifestation qui est contenue dans la manifestation ou la contient."@fr, "Relates a manifestation to a manifestation that is contained in or contains another manifestation."@en .

<http://rdaregistry.info/Elements/m/P30214>
    rdakit:instructionNumber "3.21" ;
    rdakit:toolkitDefinition "A note providing information on attributes of a carrier or carriers of a manifestation."@en, "Note fournissant de l’information sur les attributs du ou des supports matériels de la manifestation."@fr, "Una nota que proporciona información sobre los atributos del soporte o soportes de la manifestación."@es ;
    rdakit:toolkitLabel "anmärkning om bärare"@sv, "nota sobre el soporte"@es, "note on carrier"@en, "note sur le support matériel"@fr ;
    reg:hasSubproperty <http://rdaregistry.info/Elements/m/P30060>, <http://rdaregistry.info/Elements/m/P30061> ;
    reg:hasUnconstrained <http://rdaregistry.info/Elements/u/P60470> ;
    reg:lexicalAlias <http://rdaregistry.info/Elements/m/noteOnCarrier.en> ;
    reg:name "noteOnCarrier"@en ;
    reg:status <http://metadataregistry.org/uri/RegStatus/1001> ;
    a rdf:Property ;
    rdfs:domain <http://rdaregistry.info/Elements/c/C10007> ;
    rdfs:isDefinedBy <http://rdaregistry.info/Elements/m/> ;
    rdfs:label "a pour note sur le support matériel"@fr, "har anmärkning om bärare"@sv, "has note on carrier"@en ;
    skos:definition "Met une manifestation en relation avec une note fournissant de l’information sur les attributs du ou des supports matériels de la manifestation."@fr, "Relates a manifestation to a note providing information on attributes of a carrier or carriers of a manifestation."@en .

<http://rdaregistry.info/Elements/m/P30215>
    rdakit:instructionNumber "18.5" ;
    rdakit:toolkitDefinition "An agent responsible for the production of paper used to manufacture a manifestation."@en, "Personne, famille ou collectivité responsable de la production du papier utilisé pour fabriquer une manifestation."@fr, "Una persona, familia o entidad corporativa responsable de la producción del papel usado para fabricar una manifestación."@es ;
    rdakit:toolkitLabel "papermaker"@en, "papetier"@fr, "productor de papel"@es ;
    reg:hasSubproperty <http://rdaregistry.info/Elements/m/object/P30215> ;
    reg:hasUnconstrained <http://rdaregistry.info/Elements/u/P60746> ;
    reg:lexicalAlias <http://rdaregistry.info/Elements/m/papermaker.en> ;
    reg:name "papermaker"@en ;
    reg:status <http://metadataregistry.org/uri/RegStatus/1001> ;
    a rdf:Property ;
    rdfs:domain <http://rdaregistry.info/Elements/c/C10007> ;
    rdfs:isDefinedBy <http://rdaregistry.info/Elements/m/> ;
    rdfs:label "a pour papetier"@fr, "has papermaker"@en ;
    rdfs:subPropertyOf <http://rdaregistry.info/Elements/m/P30082> ;
    skos:definition "Met une manifestation en relation avec une personne, famille ou collectivité responsable de la production du papier utilisé pour fabriquer une manifestation."@fr, "Relates a manifestation to an agent responsible for the production of paper used to manufacture a manifestation."@en .

<http://rdaregistry.info/Elements/m/P30216>
    rdakit:instructionNumber "3.7.1.4" ;
    rdakit:toolkitDefinition "Details of a physical or chemical substance applied to a base material of a manifestation."@en, "Detalles de una sustancia física o química aplicada al material de base de un recurso."@es ;
    rdakit:toolkitLabel "details of applied material"@en, "detaljerad information om applicerat material"@sv, "detalles del material aplicado"@es ;
    reg:hasSubproperty <http://rdaregistry.info/Elements/m/P30223> ;
    reg:hasUnconstrained <http://rdaregistry.info/Elements/u/P60767> ;
    reg:lexicalAlias <http://rdaregistry.info/Elements/m/detailsOfAppliedMaterial.en> ;
    reg:name "detailsOfAppliedMaterial"@en ;
    reg:status <http://metadataregistry.org/uri/RegStatus/1001> ;
    a rdf:Property ;
    rdfs:domain <http://rdaregistry.info/Elements/c/C10007> ;
    rdfs:isDefinedBy <http://rdaregistry.info/Elements/m/> ;
    rdfs:label "har detaljerad information om applicerat material"@sv, "has details of applied material"@en ;
    skos:definition "Relates a manifestation to details of a physical or chemical substance applied to a base material of a manifestation."@en .

<http://rdaregistry.info/Elements/m/P30217>
    rdakit:instructionNumber "3.6.1.4" ;
    rdakit:toolkitDefinition "Details of an underlying physical material of a manifestation."@en, "Detalles del material físico que sostiene el recurso."@es ;
    rdakit:toolkitLabel "details of base material"@en, "detaljerad information om bärande matieral"@sv, "detalles del material de base"@es ;
    reg:hasUnconstrained <http://rdaregistry.info/Elements/u/P60768> ;
    reg:lexicalAlias <http://rdaregistry.info/Elements/m/detailsOfBaseMaterial.en> ;
    reg:name "detailsOfBaseMaterial"@en ;
    reg:status <http://metadataregistry.org/uri/RegStatus/1001> ;
    a rdf:Property ;
    rdfs:domain <http://rdaregistry.info/Elements/c/C10007> ;
    rdfs:isDefinedBy <http://rdaregistry.info/Elements/m/> ;
    rdfs:label "har detaljerad information om bärande matieral"@sv, "has details of base material"@en ;
    skos:definition "Relates a manifestation to details of an underlying physical material of a manifestation."@en .

<http://rdaregistry.info/Elements/m/P30218>
    rdakit:instructionNumber "3.12.1.4" ;
    rdakit:toolkitDefinition "Details of a proportional relationship between a whole sheet in a printed or manuscript resource, and the individual leaves that result if that sheet is left full, cut, or folded."@en, "Detalles del resultado del plegado de una hoja impresa para formar un conjunto de hojas (por ej., una hoja doblada una vez para formar un folio, dos veces para formar un cuarto, tres veces para formar un octavo)."@es ;
    rdakit:toolkitLabel "details of bibliographic format"@en, "detaljerad information om bokformat"@sv, "detalles del formato libro"@es ;
    reg:hasUnconstrained <http://rdaregistry.info/Elements/u/P60769> ;
    reg:lexicalAlias <http://rdaregistry.info/Elements/m/detailsOfBibliographicFormat.en> ;
    reg:name "detailsOfBibliographicFormat"@en ;
    reg:status <http://metadataregistry.org/uri/RegStatus/1001> ;
    a rdf:Property ;
    rdfs:domain <http://rdaregistry.info/Elements/c/C10007> ;
    rdfs:isDefinedBy <http://rdaregistry.info/Elements/m/> ;
    rdfs:label "har detaljerad information om bokformat"@sv, "has details of bibliographic format"@en ;
    skos:definition "Relates a manifestation to details of a proportional relationship between a whole sheet in a printed or manuscript resource, and the individual leaves that result if that sheet is left full, cut, or folded."@en .

<http://rdaregistry.info/Elements/m/P30219>
    rdakit:instructionNumber "3.18.3.4" ;
    rdakit:toolkitDefinition "Details of a system used to format a manifestation of a video for television broadcast."@en, "Detalles de un sistema utilizado para formatear un recurso de vídeo para transmisión por televisión."@es ;
    rdakit:toolkitLabel "details of broadcast standard"@en, "detaljerad information om sändningsstandard"@sv, "detalles de la norma de transmisión"@es ;
    reg:hasUnconstrained <http://rdaregistry.info/Elements/u/P60770> ;
    reg:lexicalAlias <http://rdaregistry.info/Elements/m/detailsOfBroadcastStandard.en> ;
    reg:name "detailsOfBroadcastStandard"@en ;
    reg:status <http://metadataregistry.org/uri/RegStatus/1001> ;
    a rdf:Property ;
    rdfs:domain <http://rdaregistry.info/Elements/c/C10007> ;
    rdfs:isDefinedBy <http://rdaregistry.info/Elements/m/> ;
    rdfs:label "har detaljerad information om sändningsstandard"@sv, "has details of broadcast standard"@en ;
    rdfs:subPropertyOf <http://rdaregistry.info/Elements/m/P30250> ;
    skos:definition "Relates a manifestation to details of a system used to format a manifestation of a video for television broadcast."@en .

<http://rdaregistry.info/Elements/m/P30220>
    rdakit:instructionNumber "3.16.8.4" ;
    rdakit:toolkitDefinition "Details of a number of sound channels used to make a recording."@en, "Detalles del número de canales sonoros utilizados para hacer una grabación (por ej., un canal para una grabación monofónica, dos canales para una grabación estereofónica)."@es ;
    rdakit:toolkitLabel "details of configuration of playback channels"@en, "detaljerad information om antal ljudkanaler"@sv, "detalles de la configuración de canales de reproducción"@es ;
    reg:hasUnconstrained <http://rdaregistry.info/Elements/u/P60771> ;
    reg:lexicalAlias <http://rdaregistry.info/Elements/m/detailsOfConfigurationOfPlaybackChannels.en> ;
    reg:name "detailsOfConfigurationOfPlaybackChannels"@en ;
    reg:status <http://metadataregistry.org/uri/RegStatus/1001> ;
    a rdf:Property ;
    rdfs:domain <http://rdaregistry.info/Elements/c/C10007> ;
    rdfs:isDefinedBy <http://rdaregistry.info/Elements/m/> ;
    rdfs:label "har detaljerad information om antal ljudkanaler"@sv, "has details of configuration of playback channels"@en ;
    rdfs:subPropertyOf <http://rdaregistry.info/Elements/m/P30245> ;
    skos:definition "Relates a manifestation to details of a number of sound channels used to make a recording."@en .

<http://rdaregistry.info/Elements/m/P30221>
    rdakit:instructionNumber "3.19.1.4" ;
    rdakit:toolkitDefinition "Details of a technical specification relating to the digital encoding of text, image, audio, video, and other types of data in a manifestation."@en, "Detalles de especificaciones técnicas relacionadas con la codificación digital de un texto, imagen, audio, vídeo y otros tipos de datos en un recurso."@es ;
    rdakit:toolkitLabel "details of digital file characteristic"@en, "detaljerad information om egenskaper för resursens digitala kodning"@sv, "detalles de las características del archivo digital"@es ;
    reg:hasSubproperty <http://rdaregistry.info/Elements/m/P30222>, <http://rdaregistry.info/Elements/m/P30224>, <http://rdaregistry.info/Elements/m/P30225> ;
    reg:hasUnconstrained <http://rdaregistry.info/Elements/u/P60772> ;
    reg:lexicalAlias <http://rdaregistry.info/Elements/m/detailsOfDigitalFileCharacteristic.en> ;
    reg:name "detailsOfDigitalFileCharacteristic"@en ;
    reg:status <http://metadataregistry.org/uri/RegStatus/1001> ;
    a rdf:Property ;
    rdfs:domain <http://rdaregistry.info/Elements/c/C10007> ;
    rdfs:isDefinedBy <http://rdaregistry.info/Elements/m/> ;
    rdfs:label "har detaljerad information om egenskaper för resursens digitala kodning"@sv, "has details of digital file characteristic"@en ;
    skos:definition "Relates a manifestation to details of a technical specification relating to the digital encoding of text, image, audio, video, and other types of data in a manifestation."@en .

<http://rdaregistry.info/Elements/m/P30222>
    rdakit:instructionNumber "3.19.8.4" ;
    rdakit:toolkitDefinition "Details of an encoding of geospatial information in a manifestation."@en, "Detalles de la codificación de información geoespacial en un recurso cartográfico (p. ej., el nivel topológico, compresión)."@es ;
    rdakit:toolkitLabel "details of digital representation of cartographic content"@en, "detaljerad information om geografisk data relaterad till kodningen av en kartografisk resurs"@sv, "detalles de la representación digital de contenido cartográfico"@es ;
    reg:hasUnconstrained <http://rdaregistry.info/Elements/u/P60773> ;
    reg:lexicalAlias <http://rdaregistry.info/Elements/m/detailsOfDigitalRepresentationOfCartographicContent.en> ;
    reg:name "detailsOfDigitalRepresentationOfCartographicContent"@en ;
    reg:status <http://metadataregistry.org/uri/RegStatus/1001> ;
    a rdf:Property ;
    rdfs:domain <http://rdaregistry.info/Elements/c/C10007> ;
    rdfs:isDefinedBy <http://rdaregistry.info/Elements/m/> ;
    rdfs:label "har detaljerad information om geografisk data relaterad till kodningen av en kartografisk resurs"@sv, "has details of digital representation of cartographic content"@en ;
    rdfs:subPropertyOf <http://rdaregistry.info/Elements/m/P30221> ;
    skos:definition "Relates a manifestation to details of an encoding of geospatial information in a manifestation."@en .

<http://rdaregistry.info/Elements/m/P30223>
    rdakit:instructionNumber "3.7.2.4" ;
    rdakit:toolkitDefinition "Details of a suspension of light-sensitive chemicals used as a coating on a microfilm or microfiche."@en, "Detalles de la suspensión de químicos suaves utilizados como cobertura en un microfilme o una microficha (por ej., haluro de plata)."@es ;
    rdakit:toolkitLabel "details of emulsion on microfilm and microfiche"@en, "detaljerad information om emulsion på microfilm och microfiche"@sv, "detalles de la emulsión en el microfilme y la microficha"@es ;
    reg:hasUnconstrained <http://rdaregistry.info/Elements/u/P60774> ;
    reg:lexicalAlias <http://rdaregistry.info/Elements/m/detailsOfEmulsionOnMicrofilmAndMicrofiche.en> ;
    reg:name "detailsOfEmulsionOnMicrofilmAndMicrofiche"@en ;
    reg:status <http://metadataregistry.org/uri/RegStatus/1001> ;
    a rdf:Property ;
    rdfs:domain <http://rdaregistry.info/Elements/c/C10007> ;
    rdfs:isDefinedBy <http://rdaregistry.info/Elements/m/> ;
    rdfs:label "har detaljerad information om emulsion på microfilm och microfiche"@sv, "has details of emulsion on microfilm and microfiche"@en ;
    rdfs:subPropertyOf <http://rdaregistry.info/Elements/m/P30216> ;
    skos:definition "Relates a manifestation to details of a suspension of light-sensitive chemicals used as a coating on a microfilm or microfiche."@en .

<http://rdaregistry.info/Elements/m/P30224>
    rdakit:instructionNumber "3.19.3.4" ;
    rdakit:toolkitDefinition "Details of a schema, standard, etc., used to encode the digital content of a manifestation."@en, "Detalles del esquema, estándar, etc., utilizado para codificar el contenido digital de un recurso."@es ;
    rdakit:toolkitLabel "details of encoding format"@en, "detaljerad information om kodningsformat"@sv, "detalles del formato de codificación"@es ;
    reg:hasUnconstrained <http://rdaregistry.info/Elements/u/P60775> ;
    reg:lexicalAlias <http://rdaregistry.info/Elements/m/detailsOfEncodingFormat.en> ;
    reg:name "detailsOfEncodingFormat"@en ;
    reg:status <http://metadataregistry.org/uri/RegStatus/1001> ;
    a rdf:Property ;
    rdfs:domain <http://rdaregistry.info/Elements/c/C10007> ;
    rdfs:isDefinedBy <http://rdaregistry.info/Elements/m/> ;
    rdfs:label "har detaljerad information om kodningsformat"@sv, "has details of encoding format"@en ;
    rdfs:subPropertyOf <http://rdaregistry.info/Elements/m/P30221> ;
    skos:definition "Relates a manifestation to details of a schema, standard, etc., used to encode the digital content of a manifestation."@en .

<http://rdaregistry.info/Elements/m/P30225>
    rdakit:instructionNumber "3.19.2.4" ;
    rdakit:toolkitDefinition "Details of a general type of data content encoded in a computer file."@en, "Detalles del tipo general de contenido de datos codificado en un archivo de computadora."@es ;
    rdakit:toolkitLabel "details of file type"@en, "detaljerad information om filtyp"@sv, "detalles del tipo de archivo"@es ;
    reg:hasUnconstrained <http://rdaregistry.info/Elements/u/P60776> ;
    reg:lexicalAlias <http://rdaregistry.info/Elements/m/detailsOfFileType.en> ;
    reg:name "detailsOfFileType"@en ;
    reg:status <http://metadataregistry.org/uri/RegStatus/1001> ;
    a rdf:Property ;
    rdfs:domain <http://rdaregistry.info/Elements/c/C10007> ;
    rdfs:isDefinedBy <http://rdaregistry.info/Elements/m/> ;
    rdfs:label "har detaljerad information om filtyp"@sv, "has details of file type"@en ;
    rdfs:subPropertyOf <http://rdaregistry.info/Elements/m/P30221> ;
    skos:definition "Relates a manifestation to details of a general type of data content encoded in a computer file."@en .

<http://rdaregistry.info/Elements/m/P30226>
    rdakit:instructionNumber "3.13.1.4" ;
    rdakit:toolkitDefinition "Details of a size of the type used to represent the characters and symbols in a manifestation."@en, "Detalles del tamaño del tipo utilizado para representar los caracteres y símbolos en un recurso."@es ;
    rdakit:toolkitLabel "details of font size"@en, "detaljerad information om teckenstorlek"@sv, "detalles del tamaño de la fuente"@es ;
    reg:hasUnconstrained <http://rdaregistry.info/Elements/u/P60777> ;
    reg:lexicalAlias <http://rdaregistry.info/Elements/m/detailsOfFontSize.en> ;
    reg:name "detailsOfFontSize"@en ;
    reg:status <http://metadataregistry.org/uri/RegStatus/1001> ;
    a rdf:Property ;
    rdfs:domain <http://rdaregistry.info/Elements/c/C10007> ;
    rdfs:isDefinedBy <http://rdaregistry.info/Elements/m/> ;
    rdfs:label "har detaljerad information om teckenstorlek"@sv, "has details of font size"@en ;
    skos:definition "Relates a manifestation to details of a size of the type used to represent the characters and symbols in a manifestation."@en .

<http://rdaregistry.info/Elements/m/P30227>
    rdakit:instructionNumber "3.10.2.4" ;
    rdakit:toolkitDefinition "Detalles de la relación entre un soporte de audio original y el soporte de una reproducción hecha del original (por ej., cinta maestra de duplicación, una impresión de prueba)."@es ;
    rdakit:toolkitLabel "details of generation of audio recording"@en, "detalles de la generación de la grabación sonora"@es ;
    reg:hasUnconstrained <http://rdaregistry.info/Elements/u/P60778> ;
    reg:lexicalAlias <http://rdaregistry.info/Elements/m/detailsOfGenerationOfAudioRecording.en> ;
    reg:name "detailsOfGenerationOfAudioRecording"@en ;
    reg:status <http://metadataregistry.org/uri/RegStatus/1008> ;
    a rdf:Property ;
    rdfs:domain <http://rdaregistry.info/Elements/c/C10007> ;
    rdfs:isDefinedBy <http://rdaregistry.info/Elements/m/> .

<http://rdaregistry.info/Elements/m/P30228>
    rdakit:instructionNumber "3.10.3.4" ;
    rdakit:toolkitDefinition "Detalles de la relación entre el soporte original de un recurso digital y el soporte de una reproducción del original (por ej., máster derivado)."@es ;
    rdakit:toolkitLabel "details of generation of digital resource"@en, "detalles de la generaión del recurso digital"@es ;
    reg:hasUnconstrained <http://rdaregistry.info/Elements/u/P60779> ;
    reg:lexicalAlias <http://rdaregistry.info/Elements/m/detailsOfGenerationOfDigitalResource.en> ;
    reg:name "detailsOfGenerationOfDigitalResource"@en ;
    reg:status <http://metadataregistry.org/uri/RegStatus/1008> ;
    a rdf:Property ;
    rdfs:domain <http://rdaregistry.info/Elements/c/C10007> ;
    rdfs:isDefinedBy <http://rdaregistry.info/Elements/m/> .

<http://rdaregistry.info/Elements/m/P30229>
    rdakit:instructionNumber "3.10.4.4" ;
    rdakit:toolkitDefinition "Detalles de la relación entre el soporte original de una microforma y el soporte de una reproducción hecha del original (por ej., un máster de impresión)."@es ;
    rdakit:toolkitLabel "details of generation of microform"@en, "detalles de la generación de la microforma"@es ;
    reg:hasUnconstrained <http://rdaregistry.info/Elements/u/P60780> ;
    reg:lexicalAlias <http://rdaregistry.info/Elements/m/detailsOfGenerationOfMicroform.en> ;
    reg:name "detailsOfGenerationOfMicroform"@en ;
    reg:status <http://metadataregistry.org/uri/RegStatus/1008> ;
    a rdf:Property ;
    rdfs:domain <http://rdaregistry.info/Elements/c/C10007> ;
    rdfs:isDefinedBy <http://rdaregistry.info/Elements/m/> .

<http://rdaregistry.info/Elements/m/P30230>
    rdakit:instructionNumber "3.10.5.4" ;
    rdakit:toolkitDefinition "Detalles de la relación entre un soporte original de una película cinematográfica como recurso y el soporte de la reproducción hecha del original (por ej., impreso de referencia)."@es ;
    rdakit:toolkitLabel "details of generation of motion picture film"@en, "detalles de la generación de la película cinematográfica"@es ;
    reg:hasUnconstrained <http://rdaregistry.info/Elements/u/P60781> ;
    reg:lexicalAlias <http://rdaregistry.info/Elements/m/detailsOfGenerationOfMotionPictureFilm.en> ;
    reg:name "detailsOfGenerationOfMotionPictureFilm"@en ;
    reg:status <http://metadataregistry.org/uri/RegStatus/1008> ;
    a rdf:Property ;
    rdfs:domain <http://rdaregistry.info/Elements/c/C10007> ;
    rdfs:isDefinedBy <http://rdaregistry.info/Elements/m/> .

<http://rdaregistry.info/Elements/m/P30231>
    rdakit:instructionNumber "3.10.6.4" ;
    rdakit:toolkitDefinition "Detalles de la relación entre un soporte original de un recurso en videocinta y el soporte de una reproducción hecha del original (por ej., copia de exhibición)."@es ;
    rdakit:toolkitLabel "details of generation of videotape"@en, "detalles de la generación de la videocinta"@es ;
    reg:hasUnconstrained <http://rdaregistry.info/Elements/u/P60782> ;
    reg:lexicalAlias <http://rdaregistry.info/Elements/m/detailsOfGenerationOfVideotape.en> ;
    reg:name "detailsOfGenerationOfVideotape"@en ;
    reg:status <http://metadataregistry.org/uri/RegStatus/1008> ;
    a rdf:Property ;
    rdfs:domain <http://rdaregistry.info/Elements/c/C10007> ;
    rdfs:isDefinedBy <http://rdaregistry.info/Elements/m/> .

<http://rdaregistry.info/Elements/m/P30232>
    rdakit:instructionNumber "3.16.5.4" ;
    rdakit:toolkitDefinition "Details of a groove width of an analog disc or a groove pitch of an analog cylinder."@en, "Detalles de la amplitud del surco de un disco análogo o el tono del surco de un cilindro análogo."@es ;
    rdakit:toolkitLabel "details of groove characteristic"@en, "detaljerad information om spårkaraktäristika"@sv, "detalles de las características del surco"@es ;
    reg:hasUnconstrained <http://rdaregistry.info/Elements/u/P60783> ;
    reg:lexicalAlias <http://rdaregistry.info/Elements/m/detailsOfGrooveCharacteristic.en> ;
    reg:name "detailsOfGrooveCharacteristic"@en ;
    reg:status <http://metadataregistry.org/uri/RegStatus/1001> ;
    a rdf:Property ;
    rdfs:domain <http://rdaregistry.info/Elements/c/C10007> ;
    rdfs:isDefinedBy <http://rdaregistry.info/Elements/m/> ;
    rdfs:label "har detaljerad information om spårkaraktäristika"@sv, "has details of groove characteristic"@en ;
    rdfs:subPropertyOf <http://rdaregistry.info/Elements/m/P30245> ;
    skos:definition "Relates a manifestation to details of a groove width of an analog disc or a groove pitch of an analog cylinder."@en .

<http://rdaregistry.info/Elements/m/P30233>
    rdakit:instructionNumber "3.11.1.4" ;
    rdakit:toolkitDefinition "Details of an arrangement of text, images, tactile notation, etc., in a manifestation."@en, "Detalles del arreglo del texto, imágenes, notación táctil, etc., en un recurso."@es ;
    rdakit:toolkitLabel "details of layout"@en, "detaljerad information om layout"@sv, "detalles de la presentación"@es ;
    reg:hasUnconstrained <http://rdaregistry.info/Elements/u/P60784> ;
    reg:lexicalAlias <http://rdaregistry.info/Elements/m/detailsOfLayout.en> ;
    reg:name "detailsOfLayout"@en ;
    reg:status <http://metadataregistry.org/uri/RegStatus/1001> ;
    a rdf:Property ;
    rdfs:domain <http://rdaregistry.info/Elements/c/C10007> ;
    rdfs:isDefinedBy <http://rdaregistry.info/Elements/m/> ;
    rdfs:label "har detaljerad information om layout"@sv, "has details of layout"@en ;
    skos:definition "Relates a manifestation to details of an arrangement of text, images, tactile notation, etc., in a manifestation."@en .

<http://rdaregistry.info/Elements/m/P30234>
    rdakit:instructionNumber "3.8.1.4" ;
    rdakit:toolkitDefinition "Details of a physical material used for the support or backing to which the base material of a manifestation has been attached."@en, "Detalles del material físico usado como soporte en el cual se sostiene el material base de un recurso."@es ;
    rdakit:toolkitLabel "details of mount"@en, "detaljerad information om montering"@sv, "detalles de la montura"@es ;
    reg:hasUnconstrained <http://rdaregistry.info/Elements/u/P60785> ;
    reg:lexicalAlias <http://rdaregistry.info/Elements/m/detailsOfMount.en> ;
    reg:name "detailsOfMount"@en ;
    reg:status <http://metadataregistry.org/uri/RegStatus/1001> ;
    a rdf:Property ;
    rdfs:domain <http://rdaregistry.info/Elements/c/C10007> ;
    rdfs:isDefinedBy <http://rdaregistry.info/Elements/m/> ;
    rdfs:label "har detaljerad information om montering"@sv, "has details of mount"@en ;
    skos:definition "Relates a manifestation to details of a physical material used for the support or backing to which the base material of a manifestation has been attached."@en .

<http://rdaregistry.info/Elements/m/P30235>
    rdakit:instructionNumber "3.16.4.4" ;
    rdakit:toolkitDefinition "Details of a speed at which an audio carrier must be operated to produce the sound intended."@en, "Detalles de la velocidad a la cual un soporte de audio debe ser operado para producir el sonido esperado."@es ;
    rdakit:toolkitLabel "details of playing speed"@en, "detaljerad information om uppspelningshastighet"@sv, "detalles de la velocidad de reproducción"@es ;
    reg:hasUnconstrained <http://rdaregistry.info/Elements/u/P60786> ;
    reg:lexicalAlias <http://rdaregistry.info/Elements/m/detailsOfPlayingSpeed.en> ;
    reg:name "detailsOfPlayingSpeed"@en ;
    reg:status <http://metadataregistry.org/uri/RegStatus/1001> ;
    a rdf:Property ;
    rdfs:domain <http://rdaregistry.info/Elements/c/C10007> ;
    rdfs:isDefinedBy <http://rdaregistry.info/Elements/m/> ;
    rdfs:label "har details of playing speed"@sv, "has details of playing speed"@en ;
    skos:definition "Relates a manifestation to details of a speed at which an audio carrier must be operated to produce the sound intended."@en .

<http://rdaregistry.info/Elements/m/P30236>
    rdakit:instructionNumber "3.14.1.4" ;
    rdakit:toolkitDefinition "Details of a relationship of the colours and tones in an image to the colours and tones of the object reproduced."@en, "Detalles de la relación de los colores y tonos en una imagen con los colores y tonos del objeto reproducido (por ej., positiva, negativa)."@es ;
    rdakit:toolkitLabel "details of polarity"@en, "detaljerad information om polaritet"@sv, "detalles de la polaridad"@es ;
    reg:hasUnconstrained <http://rdaregistry.info/Elements/u/P60787> ;
    reg:lexicalAlias <http://rdaregistry.info/Elements/m/detailsOfPolarity.en> ;
    reg:name "detailsOfPolarity"@en ;
    reg:status <http://metadataregistry.org/uri/RegStatus/1001> ;
    a rdf:Property ;
    rdfs:domain <http://rdaregistry.info/Elements/c/C10007> ;
    rdfs:isDefinedBy <http://rdaregistry.info/Elements/m/> ;
    rdfs:label "har detaljerad information om polaritet"@sv, "has details of polarity"@en ;
    skos:definition "Relates a manifestation to details of a relationship of the colours and tones in an image to the colours and tones of the object reproduced."@en .

<http://rdaregistry.info/Elements/m/P30237>
    rdakit:instructionNumber "3.17.2.4" ;
    rdakit:toolkitDefinition "Details of a format used in the production of a projected image."@en, "Detalles del formato utilizado en la producción de una imagen proyectada (por ej., Cinerama, IMAX)."@es ;
    rdakit:toolkitLabel "details of presentation format"@en, "detaljerad information om filmprojektionssystem"@sv, "detalles del formato de presentación"@es ;
    reg:hasUnconstrained <http://rdaregistry.info/Elements/u/P60788> ;
    reg:lexicalAlias <http://rdaregistry.info/Elements/m/detailsOfPresentationFormat.en> ;
    reg:name "detailsOfPresentationFormat"@en ;
    reg:status <http://metadataregistry.org/uri/RegStatus/1001> ;
    a rdf:Property ;
    rdfs:domain <http://rdaregistry.info/Elements/c/C10007> ;
    rdfs:isDefinedBy <http://rdaregistry.info/Elements/m/> ;
    rdfs:label "har detaljerad information om filmprojektionssystem"@sv, "has details of presentation format"@en ;
    skos:definition "Relates a manifestation to details of a format used in the production of a projected image."@en .

<http://rdaregistry.info/Elements/m/P30238>
    rdakit:instructionNumber "3.9.1.4" ;
    rdakit:toolkitDefinition "Details of a process used to produce a manifestation."@en, "Detalles del proceso utilizado para producir un recurso."@es ;
    rdakit:toolkitLabel "details of production method"@en, "detaljerad information om produktionsmetod"@sv, "detalles del método de producción"@es ;
    reg:hasUnconstrained <http://rdaregistry.info/Elements/u/P60789> ;
    reg:lexicalAlias <http://rdaregistry.info/Elements/m/detailsOfProductionMethod.en> ;
    reg:name "detailsOfProductionMethod"@en ;
    reg:status <http://metadataregistry.org/uri/RegStatus/1001> ;
    a rdf:Property ;
    rdfs:domain <http://rdaregistry.info/Elements/c/C10007> ;
    rdfs:isDefinedBy <http://rdaregistry.info/Elements/m/> ;
    rdfs:label "har detaljerad information om produktionsmetod"@sv, "has details of production method"@en ;
    skos:definition "Relates a manifestation to details of a process used to produce a manifestation."@en .

<http://rdaregistry.info/Elements/m/P30239>
    reg:hasUnconstrained <http://rdaregistry.info/Elements/u/P60790> ;
    reg:lexicalAlias <http://rdaregistry.info/Elements/m/detailsOfProductionMethodForManuscript.en> ;
    reg:name "detailsOfProductionMethodForManuscript"@en ;
    reg:status <http://metadataregistry.org/uri/RegStatus/1008> ;
    a rdf:Property ;
    rdfs:domain <http://rdaregistry.info/Elements/c/C10007> ;
    rdfs:isDefinedBy <http://rdaregistry.info/Elements/m/> .

<http://rdaregistry.info/Elements/m/P30240>
    rdakit:instructionNumber "3.9.3.4" ;
    rdakit:toolkitDefinition "Detalles del proceso utilizado para producir un recurso táctil (por ej., repujado, termoformado)."@es ;
    rdakit:toolkitLabel "detalles del método de producción de un recurso táctil"@es ;
    reg:hasUnconstrained <http://rdaregistry.info/Elements/u/P60791> ;
    reg:lexicalAlias <http://rdaregistry.info/Elements/m/detailsOfProductionMethodForTactileResource.en> ;
    reg:name "detailsOfProductionMethodForTactileResource"@en ;
    reg:status <http://metadataregistry.org/uri/RegStatus/1008> ;
    a rdf:Property ;
    rdfs:domain <http://rdaregistry.info/Elements/c/C10007> ;
    rdfs:isDefinedBy <http://rdaregistry.info/Elements/m/> .

<http://rdaregistry.info/Elements/m/P30241>
    rdakit:instructionNumber "3.17.1.4" ;
    rdakit:toolkitDefinition "Details of a technical specification relating to the projection of a motion picture film."@en, "Detalles de especificaciones técnicas relacionadas con la proyección de un largometraje."@es ;
    rdakit:toolkitLabel "details of projection characteristic of motion picture film"@en, "detaljerad informatino om projektionskarakteristika för film"@sv, "detalles de características de proyección de un largometraje"@es ;
    reg:hasSubproperty <http://rdaregistry.info/Elements/m/P30242> ;
    reg:hasUnconstrained <http://rdaregistry.info/Elements/u/P60792> ;
    reg:lexicalAlias <http://rdaregistry.info/Elements/m/detailsOfProjectionCharacteristicOfMotionPictureFilm.en> ;
    reg:name "detailsOfProjectionCharacteristicOfMotionPictureFilm"@en ;
    reg:status <http://metadataregistry.org/uri/RegStatus/1001> ;
    a rdf:Property ;
    rdfs:domain <http://rdaregistry.info/Elements/c/C10007> ;
    rdfs:isDefinedBy <http://rdaregistry.info/Elements/m/> ;
    rdfs:label "har detaljerad information om projektionskarakteristika för film"@sv, "has details of projection characteristic of motion picture film"@en ;
    skos:definition "Relates a manifestation to details of a technical specification relating to the projection of a motion picture film."@en .

<http://rdaregistry.info/Elements/m/P30242>
    rdakit:instructionNumber "3.17.3.4" ;
    rdakit:toolkitDefinition "Details of a speed at which a projected carrier must be operated to produce the moving image intended."@en, "Detalles de la velocidad a la cual un proyector debe ser operado para producir la imagen en movimiento esperada."@es ;
    rdakit:toolkitLabel "details of projection speed"@en, "detaljerad information om projektionshastighet"@sv, "detalles de la velocidad de proyección"@es ;
    reg:hasUnconstrained <http://rdaregistry.info/Elements/u/P60793> ;
    reg:lexicalAlias <http://rdaregistry.info/Elements/m/detailsOfProjectionSpeed.en> ;
    reg:name "detailsOfProjectionSpeed"@en ;
    reg:status <http://metadataregistry.org/uri/RegStatus/1001> ;
    a rdf:Property ;
    rdfs:domain <http://rdaregistry.info/Elements/c/C10007> ;
    rdfs:isDefinedBy <http://rdaregistry.info/Elements/m/> ;
    rdfs:label "har detaljerad information om projektionshastighet"@sv, "has details of projection speed"@en ;
    rdfs:subPropertyOf <http://rdaregistry.info/Elements/m/P30241> ;
    skos:definition "Relates a manifestation to details of a speed at which a projected carrier must be operated to produce the moving image intended."@en .

<http://rdaregistry.info/Elements/m/P30243>
    rdakit:instructionNumber "3.16.3.4" ;
    rdakit:toolkitDefinition "Details of a type of medium used to record sound on an audio carrier ."@en, "Detalles del tipo de medio utilizado para grabar el sonido en un soporte de audio (por ej., magnético, óptico)."@es ;
    rdakit:toolkitLabel "details of recording medium"@en, "detaljerad information om inspelningssätt"@sv, "detalles del medio de grabación"@es ;
    reg:hasUnconstrained <http://rdaregistry.info/Elements/u/P60794> ;
    reg:lexicalAlias <http://rdaregistry.info/Elements/m/detailsOfRecordingMedium.en> ;
    reg:name "detailsOfRecordingMedium"@en ;
    reg:status <http://metadataregistry.org/uri/RegStatus/1001> ;
    a rdf:Property ;
    rdfs:domain <http://rdaregistry.info/Elements/c/C10007> ;
    rdfs:isDefinedBy <http://rdaregistry.info/Elements/m/> ;
    rdfs:label "har detaljerad information om inspelningssätt"@sv, "has details of recording medium"@en ;
    rdfs:subPropertyOf <http://rdaregistry.info/Elements/m/P30245> ;
    skos:definition "Relates a manifestation to details of a type of medium used to record sound on an audio carrier."@en .

<http://rdaregistry.info/Elements/m/P30244>
    rdakit:instructionNumber "3.15.1.5.1.4" ;
    rdakit:toolkitDefinition "Details of a designation of the size of a micro-image to the original from which it was produced."@en, "Detalles del tamaño de una microimagen en relación con el original del cual se produjo."@es ;
    rdakit:toolkitLabel "details of reduction ratio designation"@en, "detaljerad information om förminskningsgrad"@sv, "detalles de la escala de reducción"@es ;
    reg:hasUnconstrained <http://rdaregistry.info/Elements/u/P60795> ;
    reg:lexicalAlias <http://rdaregistry.info/Elements/m/detailsOfReductionRatioDesignation.en> ;
    reg:name "detailsOfReductionRatioDesignation"@en ;
    reg:status <http://metadataregistry.org/uri/RegStatus/1001> ;
    a rdf:Property ;
    rdfs:domain <http://rdaregistry.info/Elements/c/C10007> ;
    rdfs:isDefinedBy <http://rdaregistry.info/Elements/m/> ;
    rdfs:label "har detaljerad information om förminskningsgrad"@sv, "has details of reduction ratio designation"@en ;
    skos:definition "Relates a manifestation to details of a general designation of the size of a micro-image to the original from which it was produced."@en .

<http://rdaregistry.info/Elements/m/P30245>
    rdakit:instructionNumber "3.16.1.4" ;
    rdakit:toolkitDefinition "Details of a technical specification relating to the encoding of sound in a manifestation."@en, "Detalles de especificaciones técnicas relacionadas con la codificación del sonido en un recurso."@es ;
    rdakit:toolkitLabel "details of sound characteristic"@en, "detaljerad information om ljudkaraktäristika"@sv, "detalles de las características de sonido"@es ;
    reg:hasSubproperty <http://rdaregistry.info/Elements/m/P30220>, <http://rdaregistry.info/Elements/m/P30232>, <http://rdaregistry.info/Elements/m/P30243>, <http://rdaregistry.info/Elements/m/P30246>, <http://rdaregistry.info/Elements/m/P30247>, <http://rdaregistry.info/Elements/m/P30248>, <http://rdaregistry.info/Elements/m/P30249> ;
    reg:hasUnconstrained <http://rdaregistry.info/Elements/u/P60796> ;
    reg:lexicalAlias <http://rdaregistry.info/Elements/m/detailsOfSoundCharacteristic.en> ;
    reg:name "detailsOfSoundCharacteristic"@en ;
    reg:status <http://metadataregistry.org/uri/RegStatus/1001> ;
    a rdf:Property ;
    rdfs:domain <http://rdaregistry.info/Elements/c/C10007> ;
    rdfs:isDefinedBy <http://rdaregistry.info/Elements/m/> ;
    rdfs:label "har detaljerad information om ljudkaraktäristika"@sv, "has details of sound characteristic"@en ;
    skos:definition "Relates a manifestation to details of a technical specification relating to the encoding of sound in a manifestation."@en .

<http://rdaregistry.info/Elements/m/P30246>
    rdakit:instructionNumber "3.16.9.4" ;
    rdakit:toolkitDefinition "Details of an equalization system, noise reduction system, etc., used in making an audio recording."@en, "Detalles de un sistema de ecualización, sistema de reducción del sonido, etc., utilizado en la producción de una grabación de sonido."@es ;
    rdakit:toolkitLabel "details of special playback characteristic"@en, "detaljerad information om specifika uppspelningskaraktäristika"@sv, "detalles de características especiales de reproducción"@es ;
    reg:hasUnconstrained <http://rdaregistry.info/Elements/u/P60797> ;
    reg:lexicalAlias <http://rdaregistry.info/Elements/m/detailsOfSpecialPlaybackCharacteristic.en> ;
    reg:name "detailsOfSpecialPlaybackCharacteristic"@en ;
    reg:status <http://metadataregistry.org/uri/RegStatus/1001> ;
    a rdf:Property ;
    rdfs:domain <http://rdaregistry.info/Elements/c/C10007> ;
    rdfs:isDefinedBy <http://rdaregistry.info/Elements/m/> ;
    rdfs:label "har detaljerad information om specifika uppspelningskaraktäristika"@sv, "has details of special playback characteristic"@en ;
    rdfs:subPropertyOf <http://rdaregistry.info/Elements/m/P30245> ;
    skos:definition "Relates a manifestation to details of an equalization system, noise reduction system, etc., used in making an audio recording."@en .

<http://rdaregistry.info/Elements/m/P30247>
    rdakit:instructionNumber "3.16.7.4" ;
    rdakit:toolkitDefinition "Details of a number of tracks on an audiotape."@en, "Detalles del número de pistas en una cinta de audio."@es ;
    rdakit:toolkitLabel "details of tape configuration"@en, "detaljerad information om antal spår"@sv, "detalles de la configuración de cinta"@es ;
    reg:hasUnconstrained <http://rdaregistry.info/Elements/u/P60798> ;
    reg:lexicalAlias <http://rdaregistry.info/Elements/m/detailsOfTapeConfiguration.en> ;
    reg:name "detailsOfTapeConfiguration"@en ;
    reg:status <http://metadataregistry.org/uri/RegStatus/1001> ;
    a rdf:Property ;
    rdfs:domain <http://rdaregistry.info/Elements/c/C10007> ;
    rdfs:isDefinedBy <http://rdaregistry.info/Elements/m/> ;
    rdfs:label "har detaljerad information om antal spår"@sv, "has details of tape configuration"@en ;
    rdfs:subPropertyOf <http://rdaregistry.info/Elements/m/P30245> ;
    skos:definition "Relates a manifestation to details of a number of tracks on an audiotape."@en .

<http://rdaregistry.info/Elements/m/P30248>
    rdakit:instructionNumber "3.16.6.4" ;
    rdakit:toolkitDefinition "Details of a configuration of the audio track on a sound-track film."@en, "Detalles de la configuración de la banda de sonido en una película de banda sonora (por ej., pista central)."@es ;
    rdakit:toolkitLabel "details of track configuration"@en, "detaljerad information om ljudspårskonfiguration för film"@sv, "detalles de la configuración de banda sonora"@es ;
    reg:hasUnconstrained <http://rdaregistry.info/Elements/u/P60799> ;
    reg:lexicalAlias <http://rdaregistry.info/Elements/m/detailsOfTrackConfiguration.en> ;
    reg:name "detailsOfTrackConfiguration"@en ;
    reg:status <http://metadataregistry.org/uri/RegStatus/1001> ;
    a rdf:Property ;
    rdfs:domain <http://rdaregistry.info/Elements/c/C10007> ;
    rdfs:isDefinedBy <http://rdaregistry.info/Elements/m/> ;
    rdfs:label "har detaljerad information om ljudspårskonfiguration för film"@sv, "has details of track configuration"@en ;
    rdfs:subPropertyOf <http://rdaregistry.info/Elements/m/P30245> ;
    skos:definition "Relates a manifestation to details of a configuration of the audio track on a sound-track film."@en .

<http://rdaregistry.info/Elements/m/P30249>
    rdakit:instructionNumber "3.16.2.4" ;
    rdakit:toolkitDefinition "Details of a method used to encode audio content for playback."@en, "Detalles del método utilizado para codificar el contenido sonoro para reproducción (por ej., análogo, digital)."@es ;
    rdakit:toolkitLabel "details of type of recording"@en, "detaljerad information om inspelningstyp"@sv, "detalles del tipo de grabación"@es ;
    reg:hasUnconstrained <http://rdaregistry.info/Elements/u/P60800> ;
    reg:lexicalAlias <http://rdaregistry.info/Elements/m/detailsOfTypeOfRecording.en> ;
    reg:name "detailsOfTypeOfRecording"@en ;
    reg:status <http://metadataregistry.org/uri/RegStatus/1001> ;
    a rdf:Property ;
    rdfs:domain <http://rdaregistry.info/Elements/c/C10007> ;
    rdfs:isDefinedBy <http://rdaregistry.info/Elements/m/> ;
    rdfs:label "har detaljerad information om inspelningstyp"@sv, "has details of type of recording"@en ;
    rdfs:subPropertyOf <http://rdaregistry.info/Elements/m/P30245> ;
    skos:definition "Relates a manifestation to details of a method used to encode audio content for playback."@en .

<http://rdaregistry.info/Elements/m/P30250>
    rdakit:instructionNumber "3.18.1.4" ;
    rdakit:toolkitDefinition "Details of a technical specification relating to the encoding of video images in a manifestation."@en, "Detalles de especificaciones técnicas relacionadas con la codificación de las imágenes en un recurso."@es ;
    rdakit:toolkitLabel "details of video characteristic"@en, "detaljerad information om videokaraktäristika"@sv, "detalles de características de video"@es ;
    reg:hasSubproperty <http://rdaregistry.info/Elements/m/P30219>, <http://rdaregistry.info/Elements/m/P30251> ;
    reg:hasUnconstrained <http://rdaregistry.info/Elements/u/P60801> ;
    reg:lexicalAlias <http://rdaregistry.info/Elements/m/detailsOfVideoCharacteristic.en> ;
    reg:name "detailsOfVideoCharacteristic"@en ;
    reg:status <http://metadataregistry.org/uri/RegStatus/1001> ;
    a rdf:Property ;
    rdfs:domain <http://rdaregistry.info/Elements/c/C10007> ;
    rdfs:isDefinedBy <http://rdaregistry.info/Elements/m/> ;
    rdfs:label "har detaljerad information om videokaraktäristika"@sv, "has details of video characteristic"@en ;
    skos:definition "Relates a manifestation to details of a technical specification relating to the encoding of video images in a manifestation."@en .

<http://rdaregistry.info/Elements/m/P30251>
    rdakit:instructionNumber "3.18.2.4" ;
    rdakit:toolkitDefinition "Details of a standard, etc., used to encode the analog video content of a manifestation."@en, "Detalles de la norma, etc., utilizada para codificar el contenido de vídeo análogo de un recurso."@es ;
    rdakit:toolkitLabel "details of video format"@en, "detaljerad information om videoformat"@sv, "detalles del formato de video"@es ;
    reg:hasUnconstrained <http://rdaregistry.info/Elements/u/P60802> ;
    reg:lexicalAlias <http://rdaregistry.info/Elements/m/detailsOfVideoFormat.en> ;
    reg:name "detailsOfVideoFormat"@en ;
    reg:status <http://metadataregistry.org/uri/RegStatus/1001> ;
    a rdf:Property ;
    rdfs:domain <http://rdaregistry.info/Elements/c/C10007> ;
    rdfs:isDefinedBy <http://rdaregistry.info/Elements/m/> ;
    rdfs:label "har detaljerad information om videoformat"@sv, "has details of video format"@en ;
    rdfs:subPropertyOf <http://rdaregistry.info/Elements/m/P30250> ;
    skos:definition "Relates a manifestation to details of a standard, etc., used to encode the analog video content of a manifestation."@en .

<http://rdaregistry.info/Elements/m/P30252>
    rdakit:instructionNumber "3.10.1.4" ;
    rdakit:toolkitDefinition "Details of a relationship between an original carrier and a carrier of a reproduction made from an original."@en, "Detalles de la relación entre un soporte original y el soporte de una reproducción del original (por ej., una cámara maestra de primera generación, una impresión maestra de segunda generación)."@es ;
    rdakit:toolkitLabel "details of generation"@en, "detaljerad information om generation"@sv, "detalles de generación"@es ;
    reg:hasUnconstrained <http://rdaregistry.info/Elements/u/P60803> ;
    reg:lexicalAlias <http://rdaregistry.info/Elements/m/detailsOfGeneration.en> ;
    reg:name "detailsOfGeneration"@en ;
    reg:status <http://metadataregistry.org/uri/RegStatus/1001> ;
    a rdf:Property ;
    rdfs:domain <http://rdaregistry.info/Elements/c/C10007> ;
    rdfs:isDefinedBy <http://rdaregistry.info/Elements/m/> ;
    rdfs:label "har detaljerad information om generation"@sv, "has details of generation"@en ;
    skos:definition "Relates a manifestation to details of a relationship between an original carrier and a carrier of a reproduction made from an original."@en .

<http://rdaregistry.info/Elements/m/P30253>
    rdakit:toolkitDefinition "A work that is about a manifestation."@en, "Una obra que trata sobre la manifestación."@es ;
    rdakit:toolkitLabel "materia de (manifestación)"@es, "subject of (manifestation)"@en ;
    reg:hasSubproperty <http://rdaregistry.info/Elements/m/P30254>, <http://rdaregistry.info/Elements/m/object/P30253> ;
    reg:hasUnconstrained <http://rdaregistry.info/Elements/u/P60806> ;
    reg:lexicalAlias <http://rdaregistry.info/Elements/m/subjectOfManifestation.en> ;
    reg:name "subjectOfManifestation"@en ;
    reg:status <http://metadataregistry.org/uri/RegStatus/1001> ;
    a rdf:Property ;
    rdfs:domain <http://rdaregistry.info/Elements/c/C10007> ;
    rdfs:isDefinedBy <http://rdaregistry.info/Elements/m/> ;
    rdfs:label "is subject of (manifestation)"@en ;
    rdfs:subPropertyOf <http://rdaregistry.info/Elements/w/P10283> ;
    skos:definition "Relates a manifestation to a work that is about a manifestation."@en .

<http://rdaregistry.info/Elements/m/P30254>
    rdakit:instructionNumber "23.5" ;
    rdakit:toolkitDefinition "A work that describes a described manifestation."@en, "Una obra que describe una manifestación descrita."@es, "Œuvre qui décrit une manifestation décrite."@fr ;
    rdakit:toolkitLabel "described in (manifestation)"@en, "descrita en (manifestación)"@es, "décrit dans (manifestation)"@fr ;
    reg:hasSubproperty <http://rdaregistry.info/Elements/m/P30255>, <http://rdaregistry.info/Elements/m/P30256>, <http://rdaregistry.info/Elements/m/P30257>, <http://rdaregistry.info/Elements/m/P30258>, <http://rdaregistry.info/Elements/m/P30259>, <http://rdaregistry.info/Elements/m/object/P30254> ;
    reg:hasUnconstrained <http://rdaregistry.info/Elements/u/P60215> ;
    reg:lexicalAlias <http://rdaregistry.info/Elements/m/describedInManifestation.en> ;
    reg:name "describedInManifestation"@en ;
    reg:status <http://metadataregistry.org/uri/RegStatus/1001> ;
    a rdf:Property ;
    rdfs:domain <http://rdaregistry.info/Elements/c/C10007> ;
    rdfs:isDefinedBy <http://rdaregistry.info/Elements/m/> ;
    rdfs:label "est décrit dans (manifestation)"@fr, "is described in (manifestation)"@en ;
    rdfs:subPropertyOf <http://rdaregistry.info/Elements/m/P30253> ;
    skos:definition "Met une manifestation en relation avec une œuvre qui décrit une manifestation décrite."@fr, "Relates a manifestation to a work that describes a described manifestation."@en .

<http://rdaregistry.info/Elements/m/P30255>
    rdakit:instructionNumber "23.5" ;
    rdakit:toolkitDefinition "A work that examines a source manifestation to identify its components and their relations."@en, "Una obra que examina la manifestación fuente para identificar sus componentes y sus relaciones."@es, "Œuvre qui examine la manifestation source pour identifier ses composantes et leurs relations."@fr ;
    rdakit:toolkitLabel "analizada en (manifestación)"@es, "analysed in (manifestation)"@en, "analysé dans (manifestation)"@fr ;
    reg:hasSubproperty <http://rdaregistry.info/Elements/m/object/P30255> ;
    reg:hasUnconstrained <http://rdaregistry.info/Elements/u/P60219> ;
    reg:lexicalAlias <http://rdaregistry.info/Elements/m/analysedInManifestation.en> ;
    reg:name "analysedInManifestation"@en ;
    reg:status <http://metadataregistry.org/uri/RegStatus/1001> ;
    a rdf:Property ;
    rdfs:domain <http://rdaregistry.info/Elements/c/C10007> ;
    rdfs:isDefinedBy <http://rdaregistry.info/Elements/m/> ;
    rdfs:label "est analysé dans (manifestation)"@fr, "is analysed in (manifestation)"@en ;
    rdfs:subPropertyOf <http://rdaregistry.info/Elements/m/P30254> ;
    skos:definition "Met une manifestation en relation avec une œuvre qui examine la manifestation source pour identifier ses composantes et leurs relations."@fr, "Relates a manifestation to a work that examines a source manifestation to identify its components and their relations."@en .

<http://rdaregistry.info/Elements/m/P30256>
    rdakit:instructionNumber "23.5" ;
    rdakit:toolkitDefinition "A work that contains a set of explanatory or critical notes on a described manifestation."@en, "Una obra que contiene un conjunto de notas explicativas o críticas sobre la manifestación descrita."@es, "Œuvre qui contient un ensemble de notes explicatives ou critiques sur la manifestation décrite."@fr ;
    rdakit:toolkitLabel "comentario en (manifestación)"@es, "commentaire dans (manifestation)"@fr, "commentary in (manifestation)"@en ;
    reg:hasSubproperty <http://rdaregistry.info/Elements/m/object/P30256> ;
    reg:hasUnconstrained <http://rdaregistry.info/Elements/u/P60213> ;
    reg:lexicalAlias <http://rdaregistry.info/Elements/m/commentaryInManifestation.en> ;
    reg:name "commentaryInManifestation"@en ;
    reg:status <http://metadataregistry.org/uri/RegStatus/1001> ;
    a rdf:Property ;
    rdfs:domain <http://rdaregistry.info/Elements/c/C10007> ;
    rdfs:isDefinedBy <http://rdaregistry.info/Elements/m/> ;
    rdfs:label "est le commentaire dans (manifestation)"@fr, "is commentary in (manifestation)"@en ;
    rdfs:subPropertyOf <http://rdaregistry.info/Elements/m/P30254> ;
    skos:definition "Met une manifestation en relation avec une œuvre qui contient un ensemble de notes explicatives ou critiques sur la manifestation décrite."@fr, "Relates a manifestation to a work that contains a set of explanatory or critical notes on a described manifestation."@en .

<http://rdaregistry.info/Elements/m/P30257>
    rdakit:instructionNumber "23.5" ;
    rdakit:toolkitDefinition "A work that contains a critical evaluation of a described manifestation."@en, "Una obra que contiene una evaluación crítica de la manifestación descrita."@es, "Œuvre qui contient une évaluation critique de la manifestation décrite."@fr ;
    rdakit:toolkitLabel "critiqued in (manifestation)"@en, "critiqué dans (manifestation)"@fr, "críticada en (manifestación)"@es ;
    reg:hasSubproperty <http://rdaregistry.info/Elements/m/object/P30257> ;
    reg:hasUnconstrained <http://rdaregistry.info/Elements/u/P60212> ;
    reg:lexicalAlias <http://rdaregistry.info/Elements/m/critiquedInManifestation.en> ;
    reg:name "critiquedInManifestation"@en ;
    reg:status <http://metadataregistry.org/uri/RegStatus/1001> ;
    a rdf:Property ;
    rdfs:domain <http://rdaregistry.info/Elements/c/C10007> ;
    rdfs:isDefinedBy <http://rdaregistry.info/Elements/m/> ;
    rdfs:label "est critiqué dans (manifestation)"@fr, "is critiqued in (manifestation)"@en ;
    rdfs:subPropertyOf <http://rdaregistry.info/Elements/m/P30254> ;
    skos:definition "Met une manifestation en relation avec une œuvre qui contient une évaluation critique de la manifestation décrite."@fr, "Relates a manifestation to a work that contains a critical evaluation of a described manifestation."@en .

<http://rdaregistry.info/Elements/m/P30258>
    rdakit:instructionNumber "23.5" ;
    rdakit:toolkitDefinition "A work that examines or judges a described manifestation."@en, "Una obra que examina o juzga la manifestación descrita."@es, "Œuvre qui examine ou juge la manifestation décrite."@fr ;
    rdakit:toolkitLabel "evaluada en (manifestación)"@es, "evaluated in (manifestation)"@en, "évalué dans (manifestation)"@fr ;
    reg:hasSubproperty <http://rdaregistry.info/Elements/m/object/P30258> ;
    reg:hasUnconstrained <http://rdaregistry.info/Elements/u/P60218> ;
    reg:lexicalAlias <http://rdaregistry.info/Elements/m/evaluatedInManifestation.en> ;
    reg:name "evaluatedInManifestation"@en ;
    reg:status <http://metadataregistry.org/uri/RegStatus/1001> ;
    a rdf:Property ;
    rdfs:domain <http://rdaregistry.info/Elements/c/C10007> ;
    rdfs:isDefinedBy <http://rdaregistry.info/Elements/m/> ;
    rdfs:label "est évalué dans (manifestation)"@fr, "is evaluated in (manifestation)"@en ;
    rdfs:subPropertyOf <http://rdaregistry.info/Elements/m/P30254> ;
    skos:definition "Met une manifestation en relation avec une œuvre qui examine ou juge la manifestation décrite."@fr, "Relates a manifestation to a work that examines or judges a described manifestation."@en .

<http://rdaregistry.info/Elements/m/P30259>
    rdakit:instructionNumber "23.5" ;
    rdakit:toolkitDefinition "A work that contains a brief evaluation of a described manifestation."@en, "Una obra que contiene un evaluación breve de la manifestación descrita."@es, "Œuvre qui contient une brève évaluation de la manifestation décrite."@fr ;
    rdakit:toolkitLabel "recensé dans (manifestation)"@fr, "reseñada en (manifestación)"@es, "reviewed in (manifestation)"@en ;
    reg:hasSubproperty <http://rdaregistry.info/Elements/m/object/P30259> ;
    reg:hasUnconstrained <http://rdaregistry.info/Elements/u/P60211> ;
    reg:lexicalAlias <http://rdaregistry.info/Elements/m/reviewedInManifestation.en> ;
    reg:name "reviewedInManifestation"@en ;
    reg:status <http://metadataregistry.org/uri/RegStatus/1001> ;
    a rdf:Property ;
    rdfs:domain <http://rdaregistry.info/Elements/c/C10007> ;
    rdfs:isDefinedBy <http://rdaregistry.info/Elements/m/> ;
    rdfs:label "est recensé dans (manifestation)"@fr, "is reviewed in (manifestation)"@en ;
    rdfs:subPropertyOf <http://rdaregistry.info/Elements/m/P30254> ;
    skos:definition "Met une manifestation en relation avec une œuvre qui contient une brève évaluation de la manifestation décrite."@fr, "Relates a manifestation to a work that contains a brief evaluation of a described manifestation."@en .

<http://rdaregistry.info/Elements/m/P30260>
    rdakit:instructionNumber "2.17.14" ;
    rdakit:toolkitDefinition "A note providing information on identifiers for the manifestation not recorded as part of the identifier for a manifestation element."@en ;
    rdakit:toolkitLabel "note on identifier for manifestation"@en ;
    reg:hasUnconstrained <http://rdaregistry.info/Elements/u/P60868> ;
    reg:lexicalAlias <http://rdaregistry.info/Elements/m/noteOnIdentifierForManifestation.en> ;
    reg:name "noteOnIdentifierForManifestation"@en ;
    reg:status <http://metadataregistry.org/uri/RegStatus/1001> ;
    a rdf:Property ;
    rdfs:domain <http://rdaregistry.info/Elements/c/C10007> ;
    rdfs:isDefinedBy <http://rdaregistry.info/Elements/m/> ;
    rdfs:label "has note on identifier for manifestation"@en ;
    rdfs:subPropertyOf <http://rdaregistry.info/Elements/m/P30137> ;
    skos:definition "Relates a manifestation to a note providing information on identifiers for the manifestation not recorded as part of the identifier for a manifestation element."@en .

<http://rdaregistry.info/Elements/m/P30261>
    rdakit:instructionNumber "3.19.8.5" ;
    rdakit:toolkitDefinition "A machine-readable representation of geospatial features."@en ;
    rdakit:toolkitLabel "cartographic data type"@en ;
    reg:hasUnconstrained <http://rdaregistry.info/Elements/u/P60875> ;
    reg:lexicalAlias <http://rdaregistry.info/Elements/m/cartographicDataType.en> ;
    reg:name "cartographicDataType"@en ;
    reg:status <http://metadataregistry.org/uri/RegStatus/1001> ;
    a rdf:Property ;
    rdfs:domain <http://rdaregistry.info/Elements/c/C10007> ;
    rdfs:isDefinedBy <http://rdaregistry.info/Elements/m/> ;
    rdfs:label "has cartographic data type"@en ;
    skos:definition "Relates a manifestation to a machine-readable representation of geospatial features."@en .

<http://rdaregistry.info/Elements/m/P30262>
    rdakit:instructionNumber "3.19.8.5.4" ;
    rdakit:toolkitDefinition "Details of a machine-readable representation of geospatial features."@en ;
    rdakit:toolkitLabel "details of cartographic data type"@en ;
    reg:hasSubproperty <http://rdaregistry.info/Elements/m/object/P30262> ;
    reg:hasUnconstrained <http://rdaregistry.info/Elements/u/P60876> ;
    reg:lexicalAlias <http://rdaregistry.info/Elements/m/detailsOfCartographicDataType.en> ;
    reg:name "detailsOfCartographicDataType"@en ;
    reg:status <http://metadataregistry.org/uri/RegStatus/1001> ;
    a rdf:Property ;
    rdfs:domain <http://rdaregistry.info/Elements/c/C10007> ;
    rdfs:isDefinedBy <http://rdaregistry.info/Elements/m/> ;
    rdfs:label "has details of cartographic data type"@en ;
    skos:definition "Relates a manifestation to details of a machine-readable representation of geospatial features."@en .

<http://rdaregistry.info/Elements/m/P30263>
    rdakit:instructionNumber "3.15.1.5" ;
    rdakit:toolkitDefinition "A general designation of the size of a micro-image in relation to the original from which it was produced."@en ;
    rdakit:toolkitLabel "reduction ratio designation"@en ;
    reg:hasSubproperty <http://rdaregistry.info/Elements/m/object/P30263> ;
    reg:hasUnconstrained <http://rdaregistry.info/Elements/u/P60877> ;
    reg:lexicalAlias <http://rdaregistry.info/Elements/m/reductionRatioDesignation.en> ;
    reg:name "reductionRatioDesignation"@en ;
    reg:status <http://metadataregistry.org/uri/RegStatus/1001> ;
    a rdf:Property ;
    rdfs:domain <http://rdaregistry.info/Elements/c/C10007> ;
    rdfs:isDefinedBy <http://rdaregistry.info/Elements/m/> ;
    rdfs:label "has reduction ratio designation"@en ;
    skos:definition "Relates a manifestation to a general designation of the size of a micro-image in relation to the original from which it was produced."@en .

<http://rdaregistry.info/Elements/m/P30264>
    reg:hasSubproperty <http://rdaregistry.info/Elements/m/P30048>, <http://rdaregistry.info/Elements/m/P30140>, <http://rdaregistry.info/Elements/m/P30265>, <http://rdaregistry.info/Elements/m/P30266>, <http://rdaregistry.info/Elements/m/P30267>, <http://rdaregistry.info/Elements/m/P30272>, <http://rdaregistry.info/Elements/m/P30273>, <http://rdaregistry.info/Elements/m/P30274>, <http://rdaregistry.info/Elements/m/datatype/P30264>, <http://rdaregistry.info/Elements/m/object/P30264> ;
    reg:lexicalAlias <http://rdaregistry.info/Elements/m/relatedEntityManifestation.en> ;
    reg:name "relatedEntityManifestation"@en ;
    reg:status <http://metadataregistry.org/uri/RegStatus/1001> ;
    a rdf:Property ;
    rdfs:domain <http://rdaregistry.info/Elements/c/C10007> ;
    rdfs:isDefinedBy <http://rdaregistry.info/Elements/m/> ;
    rdfs:label "has related entity (manifestation)"@en ;
    rdfs:subPropertyOf <http://rdaregistry.info/Elements/x/P00001> ;
    skos:definition "Relates a manifestation to an entity associated with a manifestation being described."@en .

<http://rdaregistry.info/Elements/m/P30265>
    reg:hasSubproperty <http://rdaregistry.info/Elements/m/datatype/P30265>, <http://rdaregistry.info/Elements/m/object/P30265> ;
    reg:hasUnconstrained <http://rdaregistry.info/Elements/u/P60313> ;
    reg:lexicalAlias <http://rdaregistry.info/Elements/m/relatedWorkManifestation.en> ;
    reg:name "relatedWorkManifestation"@en ;
    reg:status <http://metadataregistry.org/uri/RegStatus/1001> ;
    a rdf:Property ;
    rdfs:domain <http://rdaregistry.info/Elements/c/C10007> ;
    rdfs:isDefinedBy <http://rdaregistry.info/Elements/m/> ;
    rdfs:label "has related work (manifestation)"@en ;
    rdfs:subPropertyOf <http://rdaregistry.info/Elements/m/P30264> ;
    skos:definition "Relates a manifestation to a work associated with a manifestation being described."@en .

<http://rdaregistry.info/Elements/m/P30266>
    reg:hasSubproperty <http://rdaregistry.info/Elements/m/datatype/P30266>, <http://rdaregistry.info/Elements/m/object/P30266> ;
    reg:hasUnconstrained <http://rdaregistry.info/Elements/u/P60313> ;
    reg:lexicalAlias <http://rdaregistry.info/Elements/m/relatedExpressionManifestation.en> ;
    reg:name "relatedExpressionManifestation"@en ;
    reg:status <http://metadataregistry.org/uri/RegStatus/1001> ;
    a rdf:Property ;
    rdfs:domain <http://rdaregistry.info/Elements/c/C10007> ;
    rdfs:isDefinedBy <http://rdaregistry.info/Elements/m/> ;
    rdfs:label "has related expression (manifestation)"@en ;
    rdfs:subPropertyOf <http://rdaregistry.info/Elements/m/P30264> ;
    skos:definition "Relates a manifestation to an expression associated with a manifestation being described."@en .

<http://rdaregistry.info/Elements/m/P30267>
    reg:hasSubproperty <http://rdaregistry.info/Elements/m/P30268>, <http://rdaregistry.info/Elements/m/P30271>, <http://rdaregistry.info/Elements/m/datatype/P30267>, <http://rdaregistry.info/Elements/m/object/P30267> ;
    reg:lexicalAlias <http://rdaregistry.info/Elements/m/relatedAgentManifestation.en> ;
    reg:name "relatedAgentManifestation"@en ;
    reg:status <http://metadataregistry.org/uri/RegStatus/1001> ;
    a rdf:Property ;
    rdfs:domain <http://rdaregistry.info/Elements/c/C10007> ;
    rdfs:isDefinedBy <http://rdaregistry.info/Elements/m/> ;
    rdfs:label "has related agent (manifestation)"@en ;
    rdfs:subPropertyOf <http://rdaregistry.info/Elements/m/P30264> ;
    skos:definition "Relates a manifestation to an agent associated with a manifestation being described."@en .

<http://rdaregistry.info/Elements/m/P30268>
    reg:hasSubproperty <http://rdaregistry.info/Elements/m/datatype/P30268>, <http://rdaregistry.info/Elements/m/object/P30268> ;
    reg:lexicalAlias <http://rdaregistry.info/Elements/m/relatedPersonManifestation.en> ;
    reg:name "relatedPersonManifestation"@en ;
    reg:status <http://metadataregistry.org/uri/RegStatus/1001> ;
    a rdf:Property ;
    rdfs:domain <http://rdaregistry.info/Elements/c/C10007> ;
    rdfs:isDefinedBy <http://rdaregistry.info/Elements/m/> ;
    rdfs:label "has related person (manifestation)"@en ;
    rdfs:subPropertyOf <http://rdaregistry.info/Elements/m/P30267> ;
    skos:definition "Relates a manifestation to a person associated with a manifestation being described."@en .

<http://rdaregistry.info/Elements/m/P30269>
    reg:hasSubproperty <http://rdaregistry.info/Elements/m/datatype/P30269>, <http://rdaregistry.info/Elements/m/object/P30269> ;
    reg:lexicalAlias <http://rdaregistry.info/Elements/m/relatedFamilyManifestation.en> ;
    reg:name "relatedFamilyManifestation"@en ;
    reg:status <http://metadataregistry.org/uri/RegStatus/1001> ;
    a rdf:Property ;
    rdfs:domain <http://rdaregistry.info/Elements/c/C10007> ;
    rdfs:isDefinedBy <http://rdaregistry.info/Elements/m/> ;
    rdfs:label "has related family (manifestation)"@en ;
    rdfs:subPropertyOf <http://rdaregistry.info/Elements/m/P30271> ;
    skos:definition "Relates a manifestation to a family associated with a manifestation being described."@en .

<http://rdaregistry.info/Elements/m/P30270>
    reg:hasSubproperty <http://rdaregistry.info/Elements/m/datatype/P30270>, <http://rdaregistry.info/Elements/m/object/P30270> ;
    reg:lexicalAlias <http://rdaregistry.info/Elements/m/relatedCorporateBodyManifestation.en> ;
    reg:name "relatedCorporateBodyManifestation"@en ;
    reg:status <http://metadataregistry.org/uri/RegStatus/1001> ;
    a rdf:Property ;
    rdfs:domain <http://rdaregistry.info/Elements/c/C10007> ;
    rdfs:isDefinedBy <http://rdaregistry.info/Elements/m/> ;
    rdfs:label "has related corporate body (manifestation)"@en ;
    rdfs:subPropertyOf <http://rdaregistry.info/Elements/m/P30271> ;
    skos:definition "Relates a manifestation to a corporate body associated with a manifestation being described."@en .

<http://rdaregistry.info/Elements/m/P30271>
    reg:hasSubproperty <http://rdaregistry.info/Elements/m/P30269>, <http://rdaregistry.info/Elements/m/P30270>, <http://rdaregistry.info/Elements/m/datatype/P30271>, <http://rdaregistry.info/Elements/m/object/P30271> ;
    reg:lexicalAlias <http://rdaregistry.info/Elements/m/relatedCollectiveAgentManifestation.en> ;
    reg:name "relatedCollectiveAgentManifestation"@en ;
    reg:status <http://metadataregistry.org/uri/RegStatus/1001> ;
    a rdf:Property ;
    rdfs:domain <http://rdaregistry.info/Elements/c/C10007> ;
    rdfs:isDefinedBy <http://rdaregistry.info/Elements/m/> ;
    rdfs:label "has related collective agent (manifestation)"@en ;
    rdfs:subPropertyOf <http://rdaregistry.info/Elements/m/P30267> ;
    skos:definition "Relates a manifestation to a collective agent associated with a manifestation being described."@en .

<http://rdaregistry.info/Elements/m/P30272>
    reg:hasSubproperty <http://rdaregistry.info/Elements/m/datatype/P30272>, <http://rdaregistry.info/Elements/m/object/P30272> ;
    reg:lexicalAlias <http://rdaregistry.info/Elements/m/relatedPlaceManifestation.en> ;
    reg:name "relatedPlaceManifestation"@en ;
    reg:status <http://metadataregistry.org/uri/RegStatus/1001> ;
    a rdf:Property ;
    rdfs:domain <http://rdaregistry.info/Elements/c/C10007> ;
    rdfs:isDefinedBy <http://rdaregistry.info/Elements/m/> ;
    rdfs:label "has related place (manifestation)"@en ;
    rdfs:subPropertyOf <http://rdaregistry.info/Elements/m/P30264> ;
    skos:definition "Relates a manifestation to a place associated with a manifestation being described."@en .

<http://rdaregistry.info/Elements/m/P30273>
    reg:hasSubproperty <http://rdaregistry.info/Elements/m/datatype/P30273>, <http://rdaregistry.info/Elements/m/object/P30273> ;
    reg:lexicalAlias <http://rdaregistry.info/Elements/m/relatedTimespanManifestation.en> ;
    reg:name "relatedTimespanManifestation"@en ;
    reg:status <http://metadataregistry.org/uri/RegStatus/1001> ;
    a rdf:Property ;
    rdfs:domain <http://rdaregistry.info/Elements/c/C10007> ;
    rdfs:isDefinedBy <http://rdaregistry.info/Elements/m/> ;
    rdfs:label "has related time-span (manifestation)"@en ;
    rdfs:subPropertyOf <http://rdaregistry.info/Elements/m/P30264> ;
    skos:definition "Relates a manifestation to a time-span associated with a manifestation being described."@en .

<http://rdaregistry.info/Elements/m/P30274>
    reg:hasSubproperty <http://rdaregistry.info/Elements/m/datatype/P30274>, <http://rdaregistry.info/Elements/m/object/P30274> ;
    reg:lexicalAlias <http://rdaregistry.info/Elements/m/relatedNomenManifestation.en> ;
    reg:name "relatedNomenManifestation"@en ;
    reg:status <http://metadataregistry.org/uri/RegStatus/1001> ;
    a rdf:Property ;
    rdfs:domain <http://rdaregistry.info/Elements/c/C10007> ;
    rdfs:isDefinedBy <http://rdaregistry.info/Elements/m/> ;
    rdfs:label "has related nomen (manifestation)"@en ;
    rdfs:subPropertyOf <http://rdaregistry.info/Elements/m/P30264> ;
    skos:definition "Relates a manifestation to a nomen associated with a manifestation being described."@en .

<http://rdaregistry.info/Elements/m/P30275>
    rdakit:instructionNumber "3.19.6.4" ;
    rdakit:toolkitDefinition "Details of a designation for one or more regions of the world for which a videodisc or video game carrier has been encoded, indicating that playback is restricted to a device configured to decode it."@en ;
    rdakit:toolkitLabel "details of regional encoding"@en ;
    reg:hasUnconstrained <http://rdaregistry.info/Elements/u/P60904> ;
    reg:lexicalAlias <http://rdaregistry.info/Elements/m/detailsOfRegionalEncoding.en> ;
    reg:name "detailsOfRegionalEncoding"@en ;
    reg:status <http://metadataregistry.org/uri/RegStatus/1001> ;
    a rdf:Property ;
    rdfs:domain <http://rdaregistry.info/Elements/c/C10007> ;
    rdfs:isDefinedBy <http://rdaregistry.info/Elements/m/> ;
    rdfs:label "has details of regional encoding"@en ;
    rdfs:subPropertyOf <http://rdaregistry.info/Elements/m/P30221> ;
    skos:definition "Relates a manifestation to details of a designation for one or more regions of the world for which a videodisc or video game carrier has been encoded, indicating that playback is restricted to a device configured to decode it."@en .

