@prefix rdf: <http://www.w3.org/1999/02/22-rdf-syntax-ns#> .
@prefix dc: <http://purl.org/dc/elements/1.1/> .
@prefix rdakit: <http://metadataregistry.org/uri/profile/rdakit/> .
@prefix reg: <http://metadataregistry.org/uri/profile/regap/> .
@prefix skos: <http://www.w3.org/2004/02/skos/core#> .

<http://metadataregistry.org/uri/RegStatus/1001>
    a skos:Concept ;
    skos:prefLabel "Published"@en .

<http://rdaregistry.info/termList/videoFormat>
    dc:title "RDA Video Format" ;
    a skos:ConceptScheme .

<http://rdaregistry.info/termList/videoFormat/1001>
    rdakit:toolkitDefinition "A video format for analog tape developed for consumer use by Sony in 1975."@en ;
    rdakit:toolkitLabel "Betamax"@en ;
    reg:identifier <http://metadataregistry.org/concepts/899> ;
    reg:status <http://metadataregistry.org/uri/RegStatus/1001> ;
    a skos:Concept ;
    skos:altLabel "Beta"@en ;
    skos:definition "A video format for analog tape developed for consumer use by Sony in 1975."@en ;
    skos:inScheme <http://rdaregistry.info/termList/videoFormat> ;
    skos:prefLabel "Betamax"@en .

<http://rdaregistry.info/termList/videoFormat/1002>
    rdakit:toolkitDefinition "A video format for analogue tape developed for professional use by Sony in 1982."@en ;
    rdakit:toolkitLabel "Betacam"@en ;
    reg:identifier <http://metadataregistry.org/concepts/900> ;
    reg:status <http://metadataregistry.org/uri/RegStatus/1001> ;
    a skos:Concept ;
    skos:definition "A video format for analogue tape developed for professional use by Sony in 1982."@en ;
    skos:inScheme <http://rdaregistry.info/termList/videoFormat> ;
    skos:prefLabel "Betacam"@en .

<http://rdaregistry.info/termList/videoFormat/1004>
    rdakit:toolkitDefinition "A video format for analogue disc."@en ;
    rdakit:toolkitLabel "CED"@en ;
    reg:identifier <http://metadataregistry.org/concepts/902> ;
    reg:status <http://metadataregistry.org/uri/RegStatus/1001> ;
    a skos:Concept ;
    skos:altLabel "Capacitance Electronic Disc"@en ;
    skos:definition "A video format for analogue disc."@en ;
    skos:inScheme <http://rdaregistry.info/termList/videoFormat> ;
    skos:prefLabel "CED"@en .

<http://rdaregistry.info/termList/videoFormat/1005>
    rdakit:toolkitDefinition "A video format for analogue tape developed for professional use by Ampex in 1988."@en ;
    rdakit:toolkitLabel "D-2"@en ;
    reg:identifier <http://metadataregistry.org/concepts/903> ;
    reg:status <http://metadataregistry.org/uri/RegStatus/1001> ;
    a skos:Concept ;
    skos:definition "A video format for analogue tape developed for professional use by Ampex in 1988."@en ;
    skos:inScheme <http://rdaregistry.info/termList/videoFormat> ;
    skos:prefLabel "D-2"@en .

<http://rdaregistry.info/termList/videoFormat/1006>
    rdakit:toolkitDefinition "A video format for analogue tape developed for professional use by the Electronic Industries Association of Japan in 1969."@en ;
    rdakit:toolkitLabel "EIAJ"@en ;
    reg:identifier <http://metadataregistry.org/concepts/904> ;
    reg:status <http://metadataregistry.org/uri/RegStatus/1001> ;
    a skos:Concept ;
    skos:definition "A video format for analogue tape developed for professional use by the Electronic Industries Association of Japan in 1969."@en ;
    skos:inScheme <http://rdaregistry.info/termList/videoFormat> ;
    skos:prefLabel "EIAJ"@en .

<http://rdaregistry.info/termList/videoFormat/1007>
    rdakit:toolkitDefinition "A video format for analogue and digital tape that includes Video8, Hi-8, and Digital8 formats."@en ;
    rdakit:toolkitLabel "8 mm"@en ;
    reg:identifier <http://metadataregistry.org/concepts/905> ;
    reg:status <http://metadataregistry.org/uri/RegStatus/1001> ;
    a skos:Concept ;
    skos:definition "A video format for analogue and digital tape that includes Video8, Hi-8, and Digital8 formats."@en ;
    skos:inScheme <http://rdaregistry.info/termList/videoFormat> ;
    skos:prefLabel "8 mm"@en .

<http://rdaregistry.info/termList/videoFormat/1008>
    rdakit:toolkitDefinition "A video format for analogue tape that is part of the 8 mm format."@en ;
    rdakit:toolkitLabel "Hi-8 mm"@en ;
    reg:identifier <http://metadataregistry.org/concepts/906> ;
    reg:status <http://metadataregistry.org/uri/RegStatus/1001> ;
    a skos:Concept ;
    skos:definition "A video format for analogue tape that is part of the 8 mm format."@en ;
    skos:inScheme <http://rdaregistry.info/termList/videoFormat> ;
    skos:prefLabel "Hi-8 mm"@en .

<http://rdaregistry.info/termList/videoFormat/1009>
    rdakit:toolkitDefinition "A video format for optical disc that is read by a laser."@en ;
    rdakit:toolkitLabel "Laser optical"@en ;
    reg:identifier <http://metadataregistry.org/concepts/907> ;
    reg:status <http://metadataregistry.org/uri/RegStatus/1001> ;
    a skos:Concept ;
    skos:definition "A video format for optical disc that is read by a laser."@en ;
    skos:inScheme <http://rdaregistry.info/termList/videoFormat> ;
    skos:prefLabel "Laser optical"@en .

<http://rdaregistry.info/termList/videoFormat/1010>
    rdakit:toolkitDefinition "A video format for analogue tape developed for professional use by Panasonic in 1986."@en ;
    rdakit:toolkitLabel "M-II"@en ;
    reg:identifier <http://metadataregistry.org/concepts/908> ;
    reg:status <http://metadataregistry.org/uri/RegStatus/1001> ;
    a skos:Concept ;
    skos:definition "A video format for analogue tape developed for professional use by Panasonic in 1986."@en ;
    skos:inScheme <http://rdaregistry.info/termList/videoFormat> ;
    skos:prefLabel "M-II"@en .

<http://rdaregistry.info/termList/videoFormat/1011>
    rdakit:toolkitDefinition "A video format for analogue tape developed for professional use by Ampex in 1956."@en ;
    rdakit:toolkitLabel "Quadruplex"@en ;
    reg:identifier <http://metadataregistry.org/concepts/909> ;
    reg:status <http://metadataregistry.org/uri/RegStatus/1001> ;
    a skos:Concept ;
    skos:definition "A video format for analogue tape developed for professional use by Ampex in 1956."@en ;
    skos:inScheme <http://rdaregistry.info/termList/videoFormat> ;
    skos:prefLabel "Quadruplex"@en .

<http://rdaregistry.info/termList/videoFormat/1012>
    rdakit:toolkitDefinition "A video format for analogue tape based on VHS that increases horizontal resolution to 420 lines."@en ;
    rdakit:toolkitLabel "Super-VHS"@en ;
    reg:identifier <http://metadataregistry.org/concepts/910> ;
    reg:status <http://metadataregistry.org/uri/RegStatus/1001> ;
    a skos:Concept ;
    skos:definition "A video format for analogue tape based on VHS that increases horizontal resolution to 420 lines."@en ;
    skos:inScheme <http://rdaregistry.info/termList/videoFormat> ;
    skos:prefLabel "Super-VHS"@en .

<http://rdaregistry.info/termList/videoFormat/1013>
    rdakit:toolkitDefinition "A video format for analogue tape developed for professional use by Ampex and Sony in 1976."@en ;
    rdakit:toolkitLabel "Type C"@en ;
    reg:identifier <http://metadataregistry.org/concepts/911> ;
    reg:status <http://metadataregistry.org/uri/RegStatus/1001> ;
    a skos:Concept ;
    skos:definition "A video format for analogue tape developed for professional use by Ampex and Sony in 1976."@en ;
    skos:inScheme <http://rdaregistry.info/termList/videoFormat> ;
    skos:prefLabel "Type C"@en .

<http://rdaregistry.info/termList/videoFormat/1014>
    rdakit:toolkitDefinition "A video format for analogue tape developed for professional use by Sony in 1969."@en ;
    rdakit:toolkitLabel "U-matic"@en ;
    reg:identifier <http://metadataregistry.org/concepts/912> ;
    reg:status <http://metadataregistry.org/uri/RegStatus/1001> ;
    a skos:Concept ;
    skos:definition "A video format for analogue tape developed for professional use by Sony in 1969."@en ;
    skos:inScheme <http://rdaregistry.info/termList/videoFormat> ;
    skos:prefLabel "U-matic"@en .

<http://rdaregistry.info/termList/videoFormat/1015>
    rdakit:toolkitDefinition "A video format for analogue tape developed for consumer use by JVC in the 1970s."@en ;
    rdakit:toolkitLabel "VHS"@en ;
    reg:identifier <http://metadataregistry.org/concepts/913> ;
    reg:status <http://metadataregistry.org/uri/RegStatus/1001> ;
    a skos:Concept ;
    skos:altLabel "Video Home System"@en ;
    skos:definition "A video format for analogue tape developed for consumer use by JVC in the 1970s."@en ;
    skos:inScheme <http://rdaregistry.info/termList/videoFormat> ;
    skos:prefLabel "VHS"@en .

<http://rdaregistry.info/termList/videoFormat/1016>
    rdakit:toolkitDefinition "A video format for analogue tape based on the Betacam format that increases horizontal resolution to 340 lines."@en ;
    rdakit:toolkitLabel "Betacam SP"@en ;
    reg:identifier <http://metadataregistry.org/concepts/1138> ;
    reg:status <http://metadataregistry.org/uri/RegStatus/1001> ;
    a skos:Concept ;
    skos:definition "A video format for analogue tape based on the Betacam format that increases horizontal resolution to 340 lines."@en ;
    skos:inScheme <http://rdaregistry.info/termList/videoFormat> ;
    skos:prefLabel "Betacam SP"@en .

