# baseURI: http://purl.bdrc.io/ontology/types/Material/
# imports: http://www.w3.org/2004/02/skos/core
# prefix: Material

@prefix Material: <http://purl.bdrc.io/ontology/types/Material/> .
@prefix adm: <http://purl.bdrc.io/ontology/admin/> .
@prefix bdo: <http://purl.bdrc.io/ontology/core/> .
@prefix bdr: <http://purl.bdrc.io/resource/> .
@prefix owl: <http://www.w3.org/2002/07/owl#> .
@prefix rdf: <http://www.w3.org/1999/02/22-rdf-syntax-ns#> .
@prefix rdfs: <http://www.w3.org/2000/01/rdf-schema#> .
@prefix skos: <http://www.w3.org/2004/02/skos/core#> .
@prefix xsd: <http://www.w3.org/2001/XMLSchema#> .

bdo:AppliedMaterial
  a owl:Class ;
  rdfs:label "applied material"@en ;
  adm:userTooltip "The material such as ink and so on that is used to impose writing on the base material"@en ;
  rdfs:seeAlso <http://rdaregistry.info/Elements/m/P30084> ;
  rdfs:subClassOf bdo:Material ;
  adm:translationPriority 2 ;
.
bdo:BaseMaterial
  a owl:Class ;
  adm:userTooltip "underlying physical material of a manifestation of a Work"@en ;
  rdfs:label "base material" ;
  rdfs:seeAlso <http://rdaregistry.info/Elements/m/P30208> ;
  rdfs:subClassOf bdo:Material ;
  adm:translationPriority 2 ;
.
bdo:Material
  a owl:Class ;
  adm:userTooltip "Materials include the base material on which the printing appears and the applied material such as ink and so on"@en ;
  rdfs:label "material"@en ;
  rdfs:seeAlso <http://rdaregistry.info/Elements/m/P30304> ;
  rdfs:seeAlso <http://rdaregistry.info/termList/RDAMaterial> ;
.
Material:
  a owl:Ontology ;
  owl:imports <http://www.w3.org/2004/02/skos/core> ;
.
bdr:AppliedMaterial_BlackInk
  a bdo:AppliedMaterial ;
  skos:prefLabel "black ink"@en ;
.
bdr:AppliedMaterial_GoldLeaf
  a bdo:AppliedMaterial ;
  skos:prefLabel "gold leaf"@en ;
.
bdr:AppliedMaterial_IndigoDye
  a bdo:AppliedMaterial ;
  rdfs:comment "paper dyed with indigo is called Nīlapattra in some contexts"@en ;
  skos:prefLabel "indigo dye"@en ;
  adm:translationPriority 2 ;
.
bdr:AppliedMaterial_Poison
  a bdo:AppliedMaterial ;
  rdfs:comment "poison (usually arsenic), giving a yellow hue"@en ;
  rdfs:comment "usually used to keep away insects and people who would want to take part of the manuscript and turn it into a magical tincture for consumption"@en ;
  skos:prefLabel "poison"@en ;
.
bdr:AppliedMaterial_RedInk
  a bdo:AppliedMaterial ;
  skos:prefLabel "red ink"@en ;
.
bdr:AppliedMaterial_SilverLeaf
  a bdo:AppliedMaterial ;
  skos:prefLabel "silver leaf"@en ;
.
bdr:MaterialBirchBark
  a bdr:MaterialWood ;
  skos:prefLabel "bhūrjapattra"@sa-x-iast ;
  skos:prefLabel "birch bark"@en ;
.
bdr:MaterialCardboard
  a bdo:BaseMaterial ;
  skos:prefLabel "cardboard"@en ;
.
bdr:MaterialCloth
  a bdo:BaseMaterial ;
  skos:prefLabel "cloth"@en ;
.
bdr:MaterialCoryphaPalmLeaf
  a bdr:MaterialPalmLeaf ;
  rdfs:seeAlso <http://www.wikidata.org/entity/Q856001> ;
  skos:prefLabel "palm leaf (corypha)"@en ;
.
bdr:MaterialDeshog
  a bdr:MaterialPaper ;
  rdfs:comment "paper made from bark of the Daphne bush (Daphne bholua and Daphne papyracea). Indeginous to Bhutan, distinct from the Lokta paper."@en ;
  rdfs:seeAlso <http://bhutan.ims.tuwien.ac.at/ahtcde00/c-viex/j-02-03-02-11/start.html> ;
  rdfs:seeAlso bdr:MaterialLoktaPaper ;
  rdfs:seeAlso <https://www.jstor.org/stable/23657810> ;
  skos:altLabel "dezo paper"@en ;
  skos:prefLabel "deshog paper"@en ;
.
bdr:MaterialDigital
  a bdo:BaseMaterial ;
  rdfs:comment "digital material for content which is held in digital format in the archive (:Etexts)"@en ;
  skos:prefLabel "digital material"@en ;
.
bdr:MaterialKhoiPaper
  a bdr:MaterialPaper ;
  skos:prefLabel "khoi paper"@en ;
.
bdr:MaterialLoktaPaper
  a bdr:MaterialPaper ;
  adm:sameAsWikidata <http://www.wikidata.org/entity/Q6668765> ;
  rdfs:comment "paper made from bark of the Daphne bush (Daphne bholua and Daphne papyracea). Indeginous to Nepal, distinct from the Deshog paper."@en ;
  rdfs:seeAlso bdr:MaterialDeshog ;
  skos:prefLabel "lokta paper"@en ;
.
bdr:MaterialMixed
  a bdo:BaseMaterial ;
  skos:prefLabel "mixed materials"@en ;
  adm:translationPriority 2 ;
.
bdr:MaterialMultiLayerPaper
  a bdr:MaterialPaper ;
  rdfs:comment "deprecated in favor of AppliedMaterial_Poison"@en ;
  rdfs:comment "used for some manuscripts in Nepal"@en ;
  owl:deprecated true ;
  skos:prefLabel "multi-layer paper"@en ;
.
bdr:MaterialPalmLeaf
  a bdo:BaseMaterial ;
  rdfs:subClassOf bdo:BaseMaterial ;
  skos:prefLabel "palm leaf"@en ;
.
bdr:MaterialPalmyraPalmLeaf
  a bdr:MaterialPalmLeaf ;
  rdfs:seeAlso <http://www.wikidata.org/entity/Q310912> ;
  skos:prefLabel "palm leaf (palmyra)"@en ;
.
bdr:MaterialPaper
  a bdo:BaseMaterial ;
  rdfs:subClassOf bdo:BaseMaterial ;
  skos:prefLabel "paper"@en ;
.
bdr:MaterialParchment
  a bdo:BaseMaterial ;
  rdfs:subClassOf bdo:BaseMaterial ;
  skos:prefLabel "parchment"@en ;
  skos:altLabel "animal membrane"@en ;
  owl:sameAs <http://www.wikidata.org/entity/Q226697> ;
.
bdr:MaterialRicePaper
  a bdr:MaterialPaper ;
  skos:prefLabel "rice paper"@en ;
.
bdr:MaterialSaPaper
  a bdr:MaterialPaper ;
  skos:prefLabel "sa paper"@en ;
.
bdr:MaterialStone
  a bdo:BaseMaterial ;
  skos:prefLabel "stone"@en ;
.
bdr:MaterialWood
  a bdo:BaseMaterial ;
  rdfs:subClassOf bdo:BaseMaterial ;
  skos:prefLabel "wood"@en ;
.
