@prefix dc:  <http://purl.org/dc/elements/1.1/> .
@prefix foaf:  <http://xmlns.com/foaf/0.1/> .
@prefix rdakit:  <http://metadataregistry.org/uri/profile/rdakit/> .
@prefix rdf:  <http://www.w3.org/1999/02/22-rdf-syntax-ns#> .
@prefix rdfs:  <http://www.w3.org/2000/01/rdf-schema#> .
@prefix reg:  <http://metadataregistry.org/uri/profile/regap/> .
@prefix skos:  <http://www.w3.org/2004/02/skos/core#> .

<http://rdaregistry.info/Elements/i/>
        dc:title       "RDA Item properties"@en ;
        foaf:homepage  <http://www.rdaregistry.info/Elements/i/> ;
        skos:note      "Properties derived from RDA elements with the domain of RDA Item."@en .

<http://rdaregistry.info/Elements/i/P40080>
        rdfs:isDefinedBy          <http://rdaregistry.info/Elements/i/> ;
        reg:status                <http://metadataregistry.org/uri/RegStatus/1001> ;
        rdfs:label                "has access point for item"@en ;
        reg:name                  "accessPointForItem"@en ;
        reg:lexicalAlias          <http://rdaregistry.info/Elements/i/accessPointForItem.en> ;
        rdf:type                  rdf:Property ;
        skos:definition           "Relates an item to an appellation of item in natural language that is taken from a vocabulary encoding scheme or is constructed using a string encoding scheme."@en ;
        rdfs:domain               <http://rdaregistry.info/Elements/c/C10003> ;
        rdakit:toolkitLabel       "access point for item"@en ;
        rdakit:toolkitDefinition  "An appellation of item in natural language that is taken from a vocabulary encoding scheme or is constructed using a string encoding scheme."@en ;
        rdfs:subPropertyOf        <http://rdaregistry.info/Elements/i/P40081> ;
        reg:hasUnconstrained      <http://rdaregistry.info/Elements/u/P60906> ;
        reg:hasSubproperty        <http://rdaregistry.info/Elements/i/object/P40080> ;
        rdakit:hasElementType     "3" ;
        reg:hasSubproperty        <http://rdaregistry.info/Elements/i/datatype/P40080> ;
        reg:hasSubproperty        <http://rdaregistry.info/Elements/i/P40083> ;
        reg:hasSubproperty        <http://rdaregistry.info/Elements/i/P40084> ;
        rdfs:subPropertyOf        <http://rdaregistry.info/Elements/x/P00016> ;
        rdfs:label                "a pour point d’accès d’un item"@fr ;
        skos:definition           "Met un item en relation avec une appellation d’item en langage naturel qui provient d’un schéma d’encodage de vocabulaire ou est construit à l’aide d’un schéma d’encodage de chaînes."@fr ;
        rdakit:toolkitLabel       "point d’accès d’un item"@fr ;
        rdakit:toolkitDefinition  "Appellation d’item en langage naturel qui provient d’un schéma d’encodage de vocabulaire ou est construit à l’aide d’un schéma d’encodage de chaînes."@fr ;
        reg:lexicalAlias          <http://rdaregistry.info/Elements/i/pointDaccèsDunItem.fr> .

<http://rdaregistry.info/Elements/i/P40029>
        rdfs:isDefinedBy          <http://rdaregistry.info/Elements/i/> ;
        reg:status                <http://metadataregistry.org/uri/RegStatus/1001> ;
        reg:name                  "accompaniedByItem"@en ;
        rdfs:label                "is accompanied by item"@en ;
        skos:definition           "Relates an item to an item that is brought together with another item after being issued."@en ;
        rdf:type                  rdf:Property ;
        rdfs:domain               <http://rdaregistry.info/Elements/c/C10003> ;
        rdfs:subPropertyOf        <http://rdaregistry.info/Elements/i/P40046> ;
        reg:hasSubproperty        <http://rdaregistry.info/Elements/i/P40032> ;
        reg:hasSubproperty        <http://rdaregistry.info/Elements/i/P40035> ;
        reg:hasSubproperty        <http://rdaregistry.info/Elements/i/P40036> ;
        reg:lexicalAlias          <http://rdaregistry.info/Elements/i/accompaniedByItem.en> ;
        reg:hasUnconstrained      <http://rdaregistry.info/Elements/u/P60196> ;
        rdakit:toolkitLabel       "accompanied by item"@en ;
        rdakit:toolkitDefinition  "An item that is brought together with another item after being issued."@en ;
        rdfs:label                "est accompagné d’un item"@fr ;
        skos:definition           "Met un item en relation avec un item qui est placé avec un autre item après publication."@fr ;
        rdakit:toolkitLabel       "accompagné d’un item"@fr ;
        rdakit:toolkitDefinition  "Item qui est placé avec un autre item après publication."@fr ;
        rdakit:toolkitLabel       "acompañado por (ítem)"@es ;
        rdakit:toolkitDefinition  "Un ítem que se ha unido con otro ítem después de su publicación."@es ;
        rdakit:instructionNumber  "24.5" ;
        reg:hasSubproperty        <http://rdaregistry.info/Elements/i/object/P40029> ;
        reg:name                  "đượcKèmTheoBởiBản"@vi ;
        rdfs:label                "được kèm theo bởi (bản)"@vi ;
        skos:definition           "Liên kết bản với bản đi kèm với bản khác sau khi được công bố."@vi ;
        rdakit:toolkitLabel       "được kèm theo bởi (bản)"@vi ;
        rdakit:toolkitDefinition  "Bản đi kèm với bản khác sau khi được công bố."@vi ;
        reg:name                  "ledsagetAfEksemplar"@da ;
        rdfs:label                "er ledsaget af (eksemplar)"@da ;
        reg:lexicalAlias          <http://rdaregistry.info/Elements/i/ledsagetAfEksemplar.da> ;
        skos:definition           "Relaterer et eksemplar til et eksemplar, der er ført sammen med et andet eksemplar efter udgivelse."@da ;
        rdakit:toolkitLabel       "ledsaget af (eksemplar)"@da ;
        rdakit:toolkitDefinition  "Eksemplar, der er ført sammen med et andet eksemplar efter udgivelse."@da ;
        rdfs:label                "ist begleitet von (Exemplar)"@de ;
        skos:definition           "Setzt ein Exemplar mit einem Exemplar, das mit einem anderen Exemplar nach dem Herausgeben zusammengebracht wurde, in Beziehung."@de ;
        rdakit:toolkitLabel       "Begleitet von (Exemplar)"@de ;
        rdakit:toolkitDefinition  "Ein Exemplar, das mit einem anderen Exemplar nach dem Herausgeben zusammengebracht wurde."@de ;
        reg:name                  "συνοδεύεταιΑπόΑντίτυπο"@el ;
        rdfs:label                "συνοδεύεται από (αντίτυπο)"@el ;
        reg:lexicalAlias          <http://rdaregistry.info/Elements/i/συνοδεύεταιΑπόΑντίτυπο.el> ;
        skos:definition           "Συνδέει ένα αντίτυπο με ένα αντίτυπο το οποίο συνενώνεται με ένα άλλο αντίτυπο μετά την έκδοσή του."@el ;
        rdakit:toolkitLabel       "συνοδεύεται από (αντίτυπο)"@el ;
        rdakit:toolkitDefinition  "Ένα αντίτυπο το οποίο συνενώνεται με ένα άλλο αντίτυπο μετά την έκδοσή του."@el ;
        rdfs:label                "és acompanyat per (ítem)"@ca ;
        skos:definition           "Relaciona un item amb un item aplegat amb un altre ítem després de la publicació."@ca ;
        rdakit:toolkitLabel       "acompanyat per (ítem)"@ca ;
        rdakit:toolkitDefinition  "Ítem aplegat amb un altre ítem després de la publicació."@ca ;
        reg:name                  "yhdistettyKappaleeseen"@fi ;
        rdfs:label                "yhdistetty kappaleeseen"@fi ;
        reg:lexicalAlias          <rdaa:yhdistettyKappaleeseen.fi> ;
        skos:definition           "Liittää kappaleen kappaleeseen, joka on yhdistetty toiseen kappaleeseen julkaisemisen jälkeen."@fi ;
        rdakit:toolkitLabel       "yhdistetty kappaleeseen"@fi ;
        rdakit:toolkitDefinition  "Kappale, joka on yhdistetty toiseen kappaleeseen julkaisemisen jälkeen."@fi ;
        reg:name                  "accompagnéDeItem"@fr ;
        reg:lexicalAlias          <http://rdaregistry.info/Elements/i/accompagnéDunItem.fr> ;
        rdakit:toolkitLabel       "ledsaget av (eksemplar)"@no ;
        rdakit:toolkitDefinition  "Et eksemplar som har blitt knyttet til et annet eksemplar etter utgivelse."@no ;
        rdakit:hasElementType     "2" ;
        reg:name                  "Példányáltalkísért"@hu ;
        rdfs:label                "kísér (példány)"@hu ;
        skos:definition           "Egy példányt hozzákapcsol egy olyan példányhoz, amelyet összevontak egy másik példánnyal kibocsájtás után."@hu ;
        rdakit:toolkitLabel       "kíséri (példány)"@hu ;
        rdakit:toolkitDefinition  "Egy példány, amelyet egy másik példánnyal összehoztak kiadása után."@hu ;
        skos:altLabel             "accompanying item relationship"@en .

<http://rdaregistry.info/Elements/i/P40051>
        rdfs:isDefinedBy          <http://rdaregistry.info/Elements/i/> ;
        reg:status                <http://metadataregistry.org/uri/RegStatus/1008> ;
        reg:name                  "accompanyingItemRelationship"@en ;
        rdf:type                  rdf:Property ;
        rdfs:domain               <http://rdaregistry.info/Elements/c/C10003> ;
        reg:hasSubproperty        <http://rdaregistry.info/Elements/i/P40029> ;
        reg:lexicalAlias          <http://rdaregistry.info/Elements/i/accompanyingItemRelationship.en> ;
        reg:hasUnconstrained      <http://rdaregistry.info/Elements/u/P60709> ;
        rdfs:label                "a pour relation d’item d’accompagnement"@fr ;
        skos:definition           "Met un item en relation avec un item qui accompagne ou est accompagné par un autre item."@fr ;
        rdakit:toolkitLabel       "relation d’item d’accompagnement"@fr ;
        rdakit:toolkitDefinition  "Item qui accompagne ou est accompagné par un autre item."@fr ;
        rdakit:toolkitLabel       "relaciones de ítem acompañante"@es ;
        rdakit:toolkitDefinition  "Un ítem que acompaña o está acompañado por el ítem."@es ;
        rdfs:subPropertyOf        <http://rdaregistry.info/Elements/i/P40046> ;
        rdakit:instructionNumber  "24.5" ;
        reg:hasSubproperty        <http://rdaregistry.info/Elements/i/object/P40051> ;
        reg:name                  "mốiQuanHệBảnKèmTheo"@vi ;
        rdfs:label                "có mối quan hệ bản kèm theo"@vi ;
        skos:definition           "Liên kết bản với bản lèm theo hoặc đi kèm bởi bản khác."@vi ;
        rdakit:toolkitLabel       "mối quan hệ bản kèm theo"@vi ;
        rdakit:toolkitDefinition  "Bản lèm theo hoặc đi kèm bởi bản khác."@vi ;
        reg:name                  "ledsagendeEksemplarrelation"@da ;
        rdfs:label                "har ledsagende eksemplarrelation med"@da ;
        reg:lexicalAlias          <http://rdaregistry.info/Elements/i/ledsagendeEksemplarrelation.da> ;
        skos:definition           "Relaterer et eksemplar til et eksemplar der ledsager eller er ledsaget af et eksemplar."@da ;
        rdakit:toolkitLabel       "ledsagende eksemplarrelation"@da ;
        rdakit:toolkitDefinition  "Eksemplar der ledsager eller er ledsaget af et eksemplar."@da ;
        rdfs:label                "hat begleitende Beziehungen auf Exemplarebene"@de ;
        skos:definition           "Setzt ein Exemplar mit einem Exemplar, das ein anderes Exemplar begleitet oder von einem begleitet wird, in Beziehung."@de ;
        rdakit:toolkitLabel       "Begleitende Beziehung auf Exemplarebene"@de ;
        rdakit:toolkitDefinition  "Ein Exemplar, das ein anderes Exemplar begleitet oder von einem begleitet wird."@de ;
        reg:name                  "συνοδευτικήΣχέσηΑντιτύπου"@el ;
        rdfs:label                "έχει συνοδευτική σχέση του αντιτύπου με"@el ;
        reg:lexicalAlias          <http://rdaregistry.info/Elements/i/συνοδευτικήΣχέσηΑντιτύπου.el> ;
        skos:definition           "Συνδέει ένα αντίτυπο με ένα αντίτυπο το οποίο συνοδεύει ή συνοδεύεται από κάποιο άλλο αντίτυπο."@el ;
        rdakit:toolkitLabel       "συνοδευτική σχέση του αντιτύπου"@el ;
        rdakit:toolkitDefinition  "Ένα αντίτυπο το οποίο συνοδεύει ή συνοδεύεται από κάποιο άλλο αντίτυπο."@el ;
        rdfs:label                "té com a relació d’ítem d’acompanyament"@ca ;
        skos:definition           "Relaciona un item amb un ítem que acompanya o és acompanyat per un altre ítem."@ca ;
        rdakit:toolkitLabel       "relació d’ítem d’acompanyament"@ca ;
        rdakit:toolkitDefinition  "Ítem que acompanya o és acompanyat per un altre ítem."@ca ;
        reg:name                  "suhdeYhdistettyynKappaleeseen"@fi ;
        rdfs:label                "suhde yhdistettyyn kappaleeseen"@fi ;
        reg:lexicalAlias          <rdaa:suhdeYhdistettyynKappaleeseen.fi> ;
        skos:definition           "Liittää kappaleen sellaiseen kappaleeseen, johon on yhdistetty toinen kappale tai joka on yhdistetty toiseen kappaleeseen."@fi ;
        rdakit:toolkitLabel       "suhde yhdistettyyn kappaleeseen"@fi ;
        rdakit:toolkitDefinition  "Kappale, johon on yhdistetty toinen kappale tai joka on yhdistetty toiseen kappaleeseen."@fi ;
        reg:name                  "relationDitemDaccompagnement"@fr ;
        reg:lexicalAlias          <http://rdaregistry.info/Elements/i/relationDitemDaccompagnement.fr> ;
        rdakit:toolkitLabel       "ledsagende eksemplar: relasjonstype"@no ;
        rdakit:toolkitDefinition  "Et eksemplar som ledsager eller ledsages av et annet eksemplar."@no ;
        reg:hasSubproperty        <http://rdaregistry.info/Elements/i/datatype/P40051> .

<http://rdaregistry.info/Elements/i/P40033>
        rdfs:isDefinedBy    <http://rdaregistry.info/Elements/i/> ;
        reg:status          <http://metadataregistry.org/uri/RegStatus/1008> ;
        rdf:type            rdf:Property ;
        rdfs:subPropertyOf  <http://rdaregistry.info/Elements/i/P40030> .

<http://rdaregistry.info/Elements/i/P40015>
        rdfs:isDefinedBy          <http://rdaregistry.info/Elements/i/> ;
        reg:status                <http://metadataregistry.org/uri/RegStatus/1001> ;
        reg:name                  "annotator"@en ;
        rdfs:label                "has annotator"@en ;
        skos:definition           "Relates an item to a person who adds notes and other information to an item by hand."@en ;
        rdf:type                  rdf:Property ;
        rdfs:domain               <http://rdaregistry.info/Elements/c/C10003> ;
        rdfs:subPropertyOf        <http://rdaregistry.info/Elements/i/P40112> ;
        reg:lexicalAlias          <http://rdaregistry.info/Elements/i/annotator.en> ;
        reg:hasUnconstrained      <http://rdaregistry.info/Elements/u/P60464> ;
        rdakit:toolkitLabel       "annotator"@en ;
        rdakit:toolkitDefinition  "A person who adds notes and other information to an item by hand."@en ;
        rdfs:label                "a pour annotateur"@fr ;
        skos:definition           "Met un item en relation avec une personne qui ajoute des notes ou d’autres informations à la main sur un item."@fr ;
        rdakit:toolkitLabel       "annotateur"@fr ;
        rdakit:toolkitDefinition  "Personne qui ajoute des notes ou d’autres informations à la main sur un item."@fr ;
        rdakit:toolkitLabel       "anotador"@es ;
        rdakit:toolkitDefinition  "Una persona que hace anotaciones manuscritas en un ítem."@es ;
        rdakit:instructionNumber  "18.5" ;
        reg:hasSubproperty        <http://rdaregistry.info/Elements/i/object/P40015> ;
        reg:name                  "ngườiChúThích"@vi ;
        rdfs:label                "có người chú thích"@vi ;
        skos:definition           "Liên kết bản với cá nhân người tạo chú thích bản thảo trên bản."@vi ;
        rdakit:toolkitLabel       "người chú thích"@vi ;
        rdakit:toolkitDefinition  "Cá nhân người tạo chú thích bản thảo trên bản."@vi ;
        reg:name                  "annotationsskriver"@da ;
        rdfs:label                "har annotationsskriver"@da ;
        reg:lexicalAlias          <http://rdaregistry.info/Elements/i/annotationsskriver.da> ;
        skos:definition           "Relaterer et eksemplar til en person, der laver manuskriptnotater på et eksemplar."@da ;
        rdakit:toolkitLabel       "annotationsskriver"@da ;
        rdakit:toolkitDefinition  "Person, der laver manuskriptnotater på et eksemplar."@da ;
        rdfs:label                "hat annotierende Person"@de ;
        skos:definition           "Setzt ein Exemplar mit einer Person, die handschriftlich Anmerkungen in ein Exemplar schreibt, in Beziehung."@de ;
        rdakit:toolkitLabel       "Annotierende Person"@de ;
        rdakit:toolkitDefinition  "Eine Person, die handschriftlich Anmerkungen in ein Exemplar schreibt."@de ;
        reg:name                  "υπομνηματιστής"@el ;
        rdfs:label                "έχει υπομνηματιστή"@el ;
        reg:lexicalAlias          <http://rdaregistry.info/Elements/i/υπομνηματιστής.el> ;
        skos:definition           "Συνδέει ένα αντίτυπο με ένα φυσικό πρόσωπο το οποίο δημιουργεί χειρόγραφα σχόλια/σημειώσεις σε ένα αντίτυπο."@el ;
        rdakit:toolkitLabel       "υπομνηματιστής"@el ;
        rdakit:toolkitDefinition  "Ένα φυσικό πρόσωπο το οποίο δημιουργεί χειρόγραφα σχόλια/σημειώσεις σε ένα αντίτυπο."@el ;
        rdfs:label                "té com a anotador"@ca ;
        skos:definition           "Relaciona un item amb una persona que fa anotacions manuscrites en un ítem."@ca ;
        rdakit:toolkitLabel       "anotador"@ca ;
        rdakit:toolkitDefinition  "Persona que fa anotacions manuscrites en un ítem."@ca ;
        reg:name                  "huomautustenKirjoittaja"@fi ;
        rdfs:label                "huomautusten kirjoittaja"@fi ;
        reg:lexicalAlias          <rdaa:huomautustenKirjoittaja.fi> ;
        skos:definition           "Liittää kappaleen henkilöön, joka on tehnyt omakätisesti huomautuksia kappaleeseen."@fi ;
        rdakit:toolkitLabel       "huomautusten kirjoittaja"@fi ;
        rdakit:toolkitDefinition  "Henkilö, joka on tehnyt omakätisesti huomautuksia kappaleeseen."@fi ;
        reg:name                  "annotateur"@fr ;
        reg:lexicalAlias          <http://rdaregistry.info/Elements/i/annotateur.fr> ;
        rdakit:toolkitLabel       "annoterende person"@no ;
        rdakit:toolkitDefinition  "En person som lager håndskrevne kommentarer i et eksemplar."@no ;
        rdakit:hasElementType     "2" ;
        reg:name                  "annotáló"@hu ;
        rdfs:label                "van kommentálója"@hu ;
        skos:definition           "Egy példányt hozzákapcsol egy személyhez, aki egy példányhoz kézírásos jegyzeteket fűz, azaz annotációt készít. "@hu ;
        rdakit:toolkitLabel       "kommentáló"@hu ;
        rdakit:toolkitDefinition  "Egy személy, aki kézírásos jegyzeteket fűz egy példányhoz."@hu ;
        reg:hasSubproperty        <http://rdaregistry.info/Elements/i/datatype/P40015> .

<http://rdaregistry.info/Elements/i/P40081>
        rdfs:isDefinedBy          <http://rdaregistry.info/Elements/i/> ;
        reg:status                <http://metadataregistry.org/uri/RegStatus/1001> ;
        rdf:type                  rdf:Property ;
        reg:name                  "appellationOfItem"@en ;
        rdfs:label                "has appellation of item"@en ;
        reg:lexicalAlias          <http://rdaregistry.info/Elements/i/appellationOfItem.en> ;
        skos:definition           "Relates an item to a nomen that is used within a given scheme or context to refer to an item."@en ;
        rdfs:domain               <http://rdaregistry.info/Elements/c/C10003> ;
        rdakit:toolkitLabel       "appellation of item"@en ;
        rdakit:toolkitDefinition  "A nomen that is used within a given scheme or context to refer to an item."@en ;
        rdfs:subPropertyOf        <http://rdaregistry.info/Elements/i/P40079> ;
        reg:hasUnconstrained      <http://rdaregistry.info/Elements/u/P60909> ;
        reg:hasSubproperty        <http://rdaregistry.info/Elements/i/object/P40081> ;
        reg:hasSubproperty        <http://rdaregistry.info/Elements/i/P40001> ;
        rdakit:hasElementType     "3" ;
        reg:hasSubproperty        <http://rdaregistry.info/Elements/i/datatype/P40081> ;
        reg:hasSubproperty        <http://rdaregistry.info/Elements/i/P40080> ;
        reg:hasSubproperty        <http://rdaregistry.info/Elements/i/P40082> ;
        rdfs:subPropertyOf        <http://rdaregistry.info/Elements/x/P00017> ;
        rdfs:label                "a pour appellation d’item"@fr ;
        skos:definition           "Met un item en relation avec un nomen qui est utilisé à l’intérieur d’un schéma ou d’un contexte donnés pour désigner un item."@fr ;
        rdakit:toolkitLabel       "appellation d’item"@fr ;
        rdakit:toolkitDefinition  "Nomen qui est utilisé à l’intérieur d’un schéma ou d’un contexte donnés pour désigner un item."@fr ;
        reg:lexicalAlias          <http://rdaregistry.info/Elements/i/appellationDitem.fr> .

<http://rdaregistry.info/Elements/i/P40083>
        rdfs:isDefinedBy          <http://rdaregistry.info/Elements/i/> ;
        reg:status                <http://metadataregistry.org/uri/RegStatus/1001> ;
        rdf:type                  rdf:Property ;
        reg:name                  "authorizedAccessPointForItem"@en ;
        rdfs:label                "has authorized access point for item"@en ;
        reg:lexicalAlias          <http://rdaregistry.info/Elements/i/authorizedAccessPointForItem.en> ;
        skos:definition           "Relates an item to an access point of item that is selected for preference in a specific vocabulary encoding scheme."@en ;
        rdfs:domain               <http://rdaregistry.info/Elements/c/C10003> ;
        rdakit:toolkitLabel       "authorized access point for item"@en ;
        rdakit:toolkitDefinition  "An access point of item that is selected for preference in a specific vocabulary encoding scheme."@en ;
        rdfs:subPropertyOf        <http://rdaregistry.info/Elements/i/P40080> ;
        reg:hasUnconstrained      <http://rdaregistry.info/Elements/u/P60916> ;
        reg:hasSubproperty        <http://rdaregistry.info/Elements/i/object/P40083> ;
        rdakit:hasElementType     "3" ;
        reg:hasSubproperty        <http://rdaregistry.info/Elements/i/datatype/P40083> ;
        rdfs:subPropertyOf        <http://rdaregistry.info/Elements/x/P00020> ;
        rdfs:label                "a pour point d’accès autorisé d’un item"@fr ;
        skos:definition           "Met un item en relation avec un point d’accès d’un item qui fait l’objet d’un choix privilégié dans un schéma d’encodage de vocabulaire spécifique."@fr ;
        rdakit:toolkitLabel       "point d’accès autorisé d’un item"@fr ;
        rdakit:toolkitDefinition  "Point d’accès d’un item qui fait l’objet d’un choix privilégié dans un schéma d’encodage de vocabulaire spécifique."@fr ;
        reg:lexicalAlias          <http://rdaregistry.info/Elements/i/pointDaccèsAutoriséDunItem.fr> .

<http://rdaregistry.info/Elements/i/P40016>
        rdfs:isDefinedBy          <http://rdaregistry.info/Elements/i/> ;
        reg:status                <http://metadataregistry.org/uri/RegStatus/1001> ;
        reg:name                  "autographer"@en ;
        rdfs:label                "has autographer"@en ;
        skos:definition           "Relates an item to a person whose manuscript signature appears on an item."@en ;
        rdf:type                  rdf:Property ;
        rdfs:domain               <http://rdaregistry.info/Elements/c/C10003> ;
        rdfs:subPropertyOf        <http://rdaregistry.info/Elements/i/P40112> ;
        reg:lexicalAlias          <http://rdaregistry.info/Elements/i/autographer.en> ;
        reg:hasUnconstrained      <http://rdaregistry.info/Elements/u/P60466> ;
        rdakit:toolkitLabel       "autographer"@en ;
        rdakit:toolkitDefinition  "A person whose manuscript signature appears on an item."@en ;
        rdfs:label                "a pour signataire autographe"@fr ;
        skos:definition           "Met un item en relation avec une personne dont la signature manuscrite figure sur un item."@fr ;
        rdakit:toolkitLabel       "signataire autographe"@fr ;
        rdakit:toolkitDefinition  "Personne dont la signature manuscrite figure sur un item."@fr ;
        rdakit:toolkitLabel       "firmante de autógrafo"@es ;
        rdakit:toolkitDefinition  "Una persona cuya firma manuscrita aparece en un ítem."@es ;
        rdakit:instructionNumber  "18.5" ;
        reg:hasSubproperty        <http://rdaregistry.info/Elements/i/object/P40016> ;
        reg:name                  "ngườiGhiBútTích"@vi ;
        rdfs:label                "có người ghi bút tích"@vi ;
        skos:definition           "Liên kết bản với cá nhân có chữ ký bản thảo xuất hiện trên bản."@vi ;
        rdakit:toolkitLabel       "người ghi bút tích"@vi ;
        rdakit:toolkitDefinition  "Cá nhân có chữ ký bản thảo xuất hiện trên bản."@vi ;
        reg:name                  "autografskriver"@da ;
        rdfs:label                "har autografskriver"@da ;
        reg:lexicalAlias          <http://rdaregistry.info/Elements/i/autografskriver.da> ;
        skos:definition           "Relaterer et eksemplar til en person, hvis manuskriptsignatur forekommer på et eksemplar."@da ;
        rdakit:toolkitLabel       "autografskriver"@da ;
        rdakit:toolkitDefinition  "Person, hvis manuskriptsignatur forekommer på et eksemplar."@da ;
        rdfs:label                "hat Unterzeichner"@de ;
        skos:definition           "Setzt ein Exemplar mit einer Person, deren handschriftliche Unterschrift auf einem Exemplar steht, in Beziehung."@de ;
        rdakit:toolkitLabel       "Unterzeichner"@de ;
        rdakit:toolkitDefinition  "Eine Person, deren handschriftliche Unterschrift auf einem Exemplar steht."@de ;
        reg:name                  "χειρόγραφηΥπογραφή"@el ;
        rdfs:label                "έχει χειρόγραφη υπογραφή"@el ;
        reg:lexicalAlias          <http://rdaregistry.info/Elements/i/χειρόγραφηΥπογραφή.el> ;
        skos:definition           "Συνδέει ένα αντίτυπο με ένα φυσικό πρόσωπο του οποίου η ιδιόχειρη υπογραφή υπάρχει σε ένα αντίτυπο."@el ;
        rdakit:toolkitLabel       "χειρόγραφη υπογραφή"@el ;
        rdakit:toolkitDefinition  "Ένα φυσικό πρόσωπο του οποίου η ιδιόχειρη υπογραφή υπάρχει σε ένα αντίτυπο."@el ;
        rdfs:label                "té com a signatari d’un autògraf"@ca ;
        skos:definition           "Relaciona un item amb una persona la signatura autògrafa de la qual figura en un ítem."@ca ;
        rdakit:toolkitLabel       "signatari d’un autògraf"@ca ;
        rdakit:toolkitDefinition  "Persona la signatura autògrafa de la qual figura en un ítem."@ca ;
        reg:name                  "nimikirjoituksenKirjoittaja"@fi ;
        rdfs:label                "nimikirjoituksen kirjoittaja"@fi ;
        reg:lexicalAlias          <rdaa:nimikirjoituksenKirjoittaja.fi> ;
        skos:definition           "Liittää kappaleen henkilöön, jonka omakätinen nimikirjoitus on kappaleessa."@fi ;
        rdakit:toolkitLabel       "nimikirjoituksen kirjoittaja"@fi ;
        rdakit:toolkitDefinition  "Henkilö, jonka omakätinen nimikirjoitus on kappaleessa."@fi ;
        reg:name                  "signataireAutographe"@fr ;
        reg:lexicalAlias          <http://rdaregistry.info/Elements/i/signataireAutographe.fr> ;
        rdakit:toolkitLabel       "person som signerer"@no ;
        rdakit:toolkitDefinition  "En person hvis håndskrevne signatur finnes på et eksemplar."@no ;
        rdakit:hasElementType     "2" ;
        reg:name                  "dedikáló "@hu ;
        rdfs:label                "van dedikálója"@hu ;
        skos:definition           "Egy példányt hozzákapcsol egy személyhez, akinek a kézírásos aláírása megjelenik egy példányon. "@hu ;
        rdakit:toolkitLabel       "dedikáló"@hu ;
        rdakit:toolkitDefinition  "Egy személy, akinek a kézírásos aláírása megjelenik egy példányon."@hu ;
        reg:hasSubproperty        <http://rdaregistry.info/Elements/i/datatype/P40016> .

<http://rdaregistry.info/Elements/i/P40013>
        rdfs:isDefinedBy          <http://rdaregistry.info/Elements/i/> ;
        reg:status                <http://metadataregistry.org/uri/RegStatus/1001> ;
        reg:name                  "binderAgent"@en ;
        rdfs:label                "has binder agent"@en ;
        skos:definition           "Relates an item to an agent who binds an item."@en ;
        rdf:type                  rdf:Property ;
        rdfs:domain               <http://rdaregistry.info/Elements/c/C10003> ;
        rdfs:subPropertyOf        <http://rdaregistry.info/Elements/i/P40093> ;
        reg:lexicalAlias          <http://rdaregistry.info/Elements/i/binderAgent.en> ;
        reg:hasUnconstrained      <http://rdaregistry.info/Elements/u/P60458> ;
        rdakit:toolkitLabel       "binder agent"@en ;
        rdakit:toolkitDefinition  "An agent who binds an item."@en ;
        rdfs:label                "a pour agent relieur"@fr ;
        skos:definition           "Met un item en relation avec un agent qui relie un item."@fr ;
        rdakit:toolkitLabel       "agent relieur"@fr ;
        rdakit:toolkitDefinition  "Agent qui relie un item."@fr ;
        rdakit:toolkitLabel       "encuadernador"@es ;
        rdakit:toolkitDefinition  "Una persona que encuaderna un ítem."@es ;
        rdakit:instructionNumber  "18.5" ;
        reg:hasSubproperty        <http://rdaregistry.info/Elements/i/object/P40013> ;
        reg:name                  "ngườiĐóngSách"@vi ;
        rdfs:label                "có người đóng sách"@vi ;
        skos:definition           "Liên kết bản với cá nhân người đóng một bản."@vi ;
        rdakit:toolkitLabel       "người đóng sách"@vi ;
        rdakit:toolkitDefinition  "Cá nhân người đóng một bản."@vi ;
        reg:name                  "bogbinder"@da ;
        rdfs:label                "har bogbinder"@da ;
        reg:lexicalAlias          <http://rdaregistry.info/Elements/i/bogbinder.da> ;
        skos:definition           "Relaterer et eksemplar til en person, der indbinder et eksemplar."@da ;
        rdakit:toolkitLabel       "bogbinder"@da ;
        rdakit:toolkitDefinition  "Person, der indbinder et eksemplar."@da ;
        rdfs:label                "hat Buchbinder"@de ;
        skos:definition           "Setzt ein Exemplar mit einer Person, die ein Exemplar bindet, in Beziehung."@de ;
        rdakit:toolkitLabel       "Buchbinder"@de ;
        rdakit:toolkitDefinition  "Eine Person, die ein Exemplar bindet."@de ;
        reg:name                  "βιβλιοδέτης"@el ;
        rdfs:label                "έχει βιβλιοδέτη"@el ;
        reg:lexicalAlias          <http://rdaregistry.info/Elements/i/βιβλιοδέτης.el> ;
        skos:definition           "Συνδέει ένα αντίτυπο με ένα φυσικό πρόσωπο που βιβλιοδετεί ένα αντίτυπο."@el ;
        rdakit:toolkitLabel       "βιβλιοδέτης"@el ;
        rdakit:toolkitDefinition  "Ένα φυσικό πρόσωπο που βιβλιοδετεί ένα αντίτυπο."@el ;
        rdfs:label                "té com a enquadernador"@ca ;
        skos:definition           "Relaciona un item amb una persona que enquaderna un ítem."@ca ;
        rdakit:toolkitLabel       "enquadernador"@ca ;
        rdakit:toolkitDefinition  "Persona que enquaderna un ítem."@ca ;
        reg:name                  "sitoja"@fi ;
        rdfs:label                "sitoja"@fi ;
        reg:lexicalAlias          <rdaa:sitoja.fi> ;
        skos:definition           "Liittää kappaleen henkilöön, joka on sitonut kappaleen."@fi ;
        rdakit:toolkitLabel       "sitoja"@fi ;
        rdakit:toolkitDefinition  "Henkilö, joka on sitonut kappaleen."@fi ;
        reg:name                  "relieur"@fr ;
        reg:lexicalAlias          <http://rdaregistry.info/Elements/i/agentRelieur.fr> ;
        rdakit:toolkitLabel       "bokbinder"@no ;
        rdakit:toolkitDefinition  "En person som binder inn et eksemplar."@no ;
        rdakit:hasElementType     "2" ;
        reg:name                  "könyvkötő"@hu ;
        rdfs:label                "van könyvkötője"@hu ;
        skos:definition           "Egy példányt hozzákapcsol egy személyhez, aki beköt egy példányt. "@hu ;
        rdakit:toolkitLabel       "könyvkötő"@hu ;
        rdakit:toolkitDefinition  "Egy személy, aki beköt egy példányt. "@hu ;
        reg:hasSubproperty        <http://rdaregistry.info/Elements/i/datatype/P40013> ;
        skos:altLabel             "binder"@en ;
        skos:altLabel             "relieur"@fr .

<http://rdaregistry.info/Elements/i/P40114>
        rdfs:isDefinedBy          <http://rdaregistry.info/Elements/i/> ;
        reg:status                <http://metadataregistry.org/uri/RegStatus/1001> ;
        rdfs:label                "has binder collective agent"@en ;
        reg:lexicalAlias          <http://rdaregistry.info/Elements/i/binderCollectiveAgent.en> ;
        skos:definition           "Relates an item to a collective agent who binds an item."@en ;
        rdakit:toolkitLabel       "binder collective agent"@en ;
        rdakit:toolkitDefinition  "A collective agent who binds an item."@en ;
        rdf:type                  rdf:Property ;
        reg:name                  "binderCollectiveAgent" ;
        rdfs:domain               <http://rdaregistry.info/Elements/c/C10003> ;
        rdakit:hasElementType     "2" ;
        reg:hasSubproperty        <http://rdaregistry.info/Elements/i/datatype/P40114> ;
        reg:hasSubproperty        <http://rdaregistry.info/Elements/i/object/P40114> ;
        rdfs:subPropertyOf        <http://rdaregistry.info/Elements/i/P40128> ;
        rdfs:subPropertyOf        <http://rdaregistry.info/Elements/i/P40013> ;
        reg:hasSubproperty        <http://rdaregistry.info/Elements/i/P40130> ;
        reg:hasSubproperty        <http://rdaregistry.info/Elements/i/P40146> ;
        reg:hasUnconstrained      <http://rdaregistry.info/Elements/u/P60458> ;
        rdfs:label                "a pour agent collectif relieur"@fr ;
        skos:definition           "Met un item en relation avec un agent collectif qui relie un item."@fr ;
        rdakit:toolkitLabel       "agent collectif relieur"@fr ;
        rdakit:toolkitDefinition  "Agent collectif qui relie un item."@fr ;
        reg:lexicalAlias          <http://rdaregistry.info/Elements/i/agentCollectifRelieur.fr> .

<http://rdaregistry.info/Elements/i/P40130>
        rdfs:isDefinedBy          <http://rdaregistry.info/Elements/i/> ;
        reg:status                <http://metadataregistry.org/uri/RegStatus/1001> ;
        rdfs:label                "has binder corporate body"@en ;
        reg:lexicalAlias          <http://rdaregistry.info/Elements/i/binderCorporateBody.en> ;
        skos:definition           "Relates an item to a corporate body who binds an item."@en ;
        rdakit:toolkitLabel       "binder corporate body"@en ;
        rdakit:toolkitDefinition  "A corporate body who binds an item."@en ;
        rdf:type                  rdf:Property ;
        reg:name                  "binderCorporateBody" ;
        rdfs:domain               <http://rdaregistry.info/Elements/c/C10003> ;
        rdakit:hasElementType     "2" ;
        reg:hasSubproperty        <http://rdaregistry.info/Elements/i/datatype/P40130> ;
        reg:hasSubproperty        <http://rdaregistry.info/Elements/i/object/P40130> ;
        rdfs:subPropertyOf        <http://rdaregistry.info/Elements/i/P40144> ;
        rdfs:subPropertyOf        <http://rdaregistry.info/Elements/i/P40114> ;
        reg:hasUnconstrained      <http://rdaregistry.info/Elements/u/P60458> ;
        rdfs:label                "a pour collectivité relieuse"@fr ;
        skos:definition           "Met un item en relation avec une collectivité qui relie un item."@fr ;
        rdakit:toolkitLabel       "collectivité relieuse"@fr ;
        rdakit:toolkitDefinition  "Collectivité qui relie un item."@fr ;
        reg:lexicalAlias          <http://rdaregistry.info/Elements/i/collectivitéRelieuse.fr> .

<http://rdaregistry.info/Elements/i/P40146>
        rdfs:isDefinedBy          <http://rdaregistry.info/Elements/i/> ;
        reg:status                <http://metadataregistry.org/uri/RegStatus/1001> ;
        rdfs:label                "has binder family"@en ;
        reg:lexicalAlias          <http://rdaregistry.info/Elements/i/binderFamily.en> ;
        skos:definition           "Relates an item to a family who binds an item."@en ;
        rdakit:toolkitLabel       "binder family"@en ;
        rdakit:toolkitDefinition  "A family who binds an item."@en ;
        rdf:type                  rdf:Property ;
        reg:name                  "binderFamily" ;
        rdfs:domain               <http://rdaregistry.info/Elements/c/C10003> ;
        rdakit:hasElementType     "2" ;
        reg:hasSubproperty        <http://rdaregistry.info/Elements/i/datatype/P40146> ;
        reg:hasSubproperty        <http://rdaregistry.info/Elements/i/object/P40146> ;
        rdfs:subPropertyOf        <http://rdaregistry.info/Elements/i/P40160> ;
        rdfs:subPropertyOf        <http://rdaregistry.info/Elements/i/P40114> ;
        reg:hasUnconstrained      <http://rdaregistry.info/Elements/u/P60458> ;
        rdfs:label                "a pour famille relieuse"@fr ;
        skos:definition           "Met un item en relation avec une famille qui relie un item."@fr ;
        rdakit:toolkitLabel       "famille relieuse"@fr ;
        rdakit:toolkitDefinition  "Famille qui relie un item."@fr ;
        reg:lexicalAlias          <http://rdaregistry.info/Elements/i/familleRelieuse.fr> .

<http://rdaregistry.info/Elements/i/P40098>
        rdfs:isDefinedBy          <http://rdaregistry.info/Elements/i/> ;
        reg:status                <http://metadataregistry.org/uri/RegStatus/1001> ;
        rdfs:label                "has binder person"@en ;
        reg:lexicalAlias          <http://rdaregistry.info/Elements/i/binderPerson.en> ;
        skos:definition           "Relates an item to a person who binds an item."@en ;
        rdakit:toolkitLabel       "binder person"@en ;
        rdakit:toolkitDefinition  "A person who binds an item."@en ;
        rdf:type                  rdf:Property ;
        reg:name                  "binderPerson" ;
        rdfs:domain               <http://rdaregistry.info/Elements/c/C10003> ;
        rdakit:hasElementType     "2" ;
        reg:hasSubproperty        <http://rdaregistry.info/Elements/i/datatype/P40098> ;
        reg:hasSubproperty        <http://rdaregistry.info/Elements/i/object/P40098> ;
        rdfs:subPropertyOf        <http://rdaregistry.info/Elements/i/P40112> ;
        rdfs:subPropertyOf        <http://rdaregistry.info/Elements/i/P40013> ;
        reg:hasUnconstrained      <http://rdaregistry.info/Elements/u/P60458> ;
        rdfs:label                "a pour personne relieuse"@fr ;
        skos:definition           "Met un item en relation avec une personne qui relie un item."@fr ;
        rdakit:toolkitLabel       "personne relieuse"@fr ;
        rdakit:toolkitDefinition  "Personne qui relie un item."@fr ;
        reg:lexicalAlias          <http://rdaregistry.info/Elements/i/personneRelieuse.fr> .

<http://rdaregistry.info/Elements/i/P40094>
        rdfs:isDefinedBy          <http://rdaregistry.info/Elements/i/> ;
        reg:status                <http://metadataregistry.org/uri/RegStatus/1001> ;
        rdfs:label                "has binding of item"@en ;
        reg:lexicalAlias          <http://rdaregistry.info/Elements/i/bindingOfItem.en> ;
        skos:definition           "Relates an item to a work that is a binding of an item."@en ;
        rdakit:toolkitLabel       "binding of item"@en ;
        rdakit:toolkitDefinition  "A work that is a binding of an item."@en ;
        rdf:type                  rdf:Property ;
        reg:name                  "bindingOfItem" ;
        reg:hasUnconstrained      <http://rdaregistry.info/Elements/u/P61005> ;
        rdfs:subPropertyOf        <http://rdaregistry.info/Elements/i/P40069> ;
        rdakit:hasElementType     "2" ;
        reg:hasSubproperty        <http://rdaregistry.info/Elements/i/object/P40094> ;
        reg:hasSubproperty        <http://rdaregistry.info/Elements/i/datatype/P40094> ;
        rdfs:domain               <http://rdaregistry.info/Elements/c/C10003> ;
        rdfs:label                "a pour reliure d’un item"@fr ;
        skos:definition           "Met un item en relation avec une œuvre qui consiste en une reliure d’un item."@fr ;
        rdakit:toolkitLabel       "reliure d’un item"@fr ;
        rdakit:toolkitDefinition  "Œuvre qui consiste en une reliure d’un item."@fr ;
        reg:lexicalAlias          <http://rdaregistry.info/Elements/i/reliureDunItem.fr> .

<http://rdaregistry.info/Elements/i/P40032>
        rdfs:isDefinedBy          <http://rdaregistry.info/Elements/i/> ;
        reg:status                <http://metadataregistry.org/uri/RegStatus/1001> ;
        reg:name                  "boundWith"@en ;
        rdfs:label                "is bound with"@en ;
        skos:definition           "Relates an item to an item that is physically combined or joined with an item."@en ;
        rdf:type                  rdf:Property ;
        rdfs:domain               <http://rdaregistry.info/Elements/c/C10003> ;
        rdfs:subPropertyOf        <http://rdaregistry.info/Elements/i/P40029> ;
        reg:lexicalAlias          <http://rdaregistry.info/Elements/i/boundWith.en> ;
        reg:hasUnconstrained      <http://rdaregistry.info/Elements/u/P60237> ;
        rdakit:toolkitLabel       "bound with"@en ;
        rdakit:toolkitDefinition  "An item that is physically combined or joined with an item."@en ;
        rdfs:label                "est relié avec"@fr ;
        skos:definition           "Met un item en relation avec un item qui est physiquement combiné ou joint à un item."@fr ;
        rdakit:toolkitLabel       "relié avec"@fr ;
        rdakit:toolkitDefinition  "Item qui est physiquement combiné ou joint à un item."@fr ;
        rdakit:toolkitLabel       "encuadernado con"@es ;
        rdakit:toolkitDefinition  "Un ítem que se ha incluido con la misma encuadernación que el ítem descrito."@es ;
        rdakit:instructionNumber  "24.5" ;
        reg:hasSubproperty        <http://rdaregistry.info/Elements/i/object/P40032> ;
        reg:name                  "đượcĐóngVới"@vi ;
        rdfs:label                "được đóng với"@vi ;
        skos:definition           "Liên kết bản với bản được đóng lại cùng tập đóng với bản đang được mô tả."@vi ;
        rdakit:toolkitLabel       "được đóng với"@vi ;
        rdakit:toolkitDefinition  "Bản được đóng lại cùng tập đóng với bản đang được mô tả."@vi ;
        reg:name                  "indbundetSammenMed"@da ;
        rdfs:label                "er indbundet sammen med"@da ;
        reg:lexicalAlias          <http://rdaregistry.info/Elements/i/indbundetSammenMed.da> ;
        skos:definition           "Relaterer et eksemplar til et eksemplar, der er indbundet i den samme indbinding som det eksemplar, der beskrives."@da ;
        rdakit:toolkitLabel       "indbundet sammen med"@da ;
        rdakit:toolkitDefinition  "Eksemplar, der er indbundet i den samme indbinding som det eksemplar, der beskrives."@da ;
        rdfs:label                "ist eingebunden mit"@de ;
        skos:definition           "Setzt ein Exemplar mit einem Exemplar, das in denselben Einband mit eingebunden ist, wie ein Exemplar, das beschrieben wird, in Beziehung."@de ;
        rdakit:toolkitLabel       "Eingebunden mit"@de ;
        rdakit:toolkitDefinition  "Ein Exemplar, das in denselben Einband mit eingebunden ist, wie ein Exemplar, das beschrieben wird."@de ;
        reg:name                  "δεμένοΜε"@el ;
        rdfs:label                "είναι δεμένο με"@el ;
        reg:lexicalAlias          <http://rdaregistry.info/Elements/i/δεμένοΜε.el> ;
        skos:definition           "Συνδέει ένα αντίτυπο με ένα αντίτυπο το οποίο έχει δεθεί μαζί με το περιγραφόμενο αντίτυπο."@el ;
        rdakit:toolkitLabel       "δεμένο με"@el ;
        rdakit:toolkitDefinition  "Ένα αντίτυπο το οποίο έχει δεθεί μαζί με το περιγραφόμενο αντίτυπο."@el ;
        rdfs:label                "és enquadernat amb"@ca ;
        skos:definition           "Relaciona un item amb un ítem que s’ha enquadernat amb un ítem que es descriu."@ca ;
        rdakit:toolkitLabel       "enquadernat amb"@ca ;
        rdakit:toolkitDefinition  "Ítem que s’ha enquadernat amb un ítem que es descriu."@ca ;
        reg:name                  "yhteensidottu"@fi ;
        rdfs:label                "yhteensidottu"@fi ;
        reg:lexicalAlias          <rdaa:yhteensidottu.fi> ;
        skos:definition           "Liittää kappaleen kappaleeseen, joka on sidottu yhteen kuvailtavan kappaleen kanssa."@fi ;
        rdakit:toolkitLabel       "yhteensidottu"@fi ;
        rdakit:toolkitDefinition  "Kappale, joka on sidottu yhteen kuvailtavan kappaleen kanssa."@fi ;
        reg:name                  "reliéAvec"@fr ;
        reg:lexicalAlias          <http://rdaregistry.info/Elements/i/reliéAvec.fr> ;
        rdakit:toolkitLabel       "innbundet med"@no ;
        rdakit:toolkitDefinition  "Et eksemplar som er innbundet sammen med eksemplaret som beskrives."@no ;
        rdakit:hasElementType     "2" ;
        reg:name                  "összekötve"@hu ;
        rdfs:label                "összekötve "@hu ;
        skos:definition           "Egy példányt hozzákapcsol egy olyan példányhoz, amely ugyanabba a kötésbe lett kötve, mint az éppen leírt példány. "@hu ;
        rdakit:toolkitLabel       "összekötve (egybekötve)"@hu ;
        rdakit:toolkitDefinition  "Egy példány, amelyet ugyanabba a kötésbe kötöttek, mint az éppen leírt példányt."@hu .

<http://rdaregistry.info/Elements/i/P40096>
        rdfs:isDefinedBy          <http://rdaregistry.info/Elements/i/> ;
        reg:status                <http://metadataregistry.org/uri/RegStatus/1001> ;
        rdfs:label                "has category of item"@en ;
        reg:lexicalAlias          <http://rdaregistry.info/Elements/i/categoryOfItem.en> ;
        skos:definition           "Relates an item to a type to which an item belongs."@en ;
        skos:altLabel             "type of item"@en ;
        rdakit:toolkitLabel       "category of item"@en ;
        rdakit:toolkitDefinition  "A type to which an item belongs."@en ;
        rdf:type                  rdf:Property ;
        reg:name                  "categoryOfItem" ;
        rdfs:domain               <http://rdaregistry.info/Elements/c/C10003> ;
        rdfs:subPropertyOf        <http://rdaregistry.info/Elements/x/P00029> ;
        rdakit:hasElementType     "5" ;
        reg:hasSubproperty        <http://rdaregistry.info/Elements/i/datatype/P40096> ;
        reg:hasUnconstrained      <http://rdaregistry.info/Elements/u/P60058> ;
        rdfs:label                "a pour catégorie d’item"@fr ;
        skos:definition           "Met un item en relation avec un type auquel un item appartient."@fr ;
        skos:altLabel             "type d’item"@fr ;
        rdakit:toolkitLabel       "catégorie d’item"@fr ;
        rdakit:toolkitDefinition  "Type auquel un item appartient."@fr ;
        reg:lexicalAlias          <http://rdaregistry.info/Elements/i/catégorieDitem.fr> .

<http://rdaregistry.info/Elements/i/P40005>
        rdfs:isDefinedBy          <http://rdaregistry.info/Elements/i/> ;
        reg:status                <http://metadataregistry.org/uri/RegStatus/1001> ;
        reg:name                  "collectionRegistrarAgent"@en ;
        rdfs:label                "has collection registrar agent"@en ;
        skos:definition           "Relates an item to an agent who is a curator who lists or inventories items in a collection aggregate."@en ;
        rdf:type                  rdf:Property ;
        rdfs:domain               <http://rdaregistry.info/Elements/c/C10003> ;
        rdfs:subPropertyOf        <http://rdaregistry.info/Elements/i/P40017> ;
        reg:lexicalAlias          <http://rdaregistry.info/Elements/i/collectionRegistrarAgent.en> ;
        reg:hasUnconstrained      <http://rdaregistry.info/Elements/u/P60067> ;
        rdakit:toolkitLabel       "collection registrar agent"@en ;
        rdakit:toolkitDefinition  "An agent who is a curator who lists or inventories items in a collection aggregate."@en ;
        rdfs:label                "a pour agent conservateur de collection"@fr ;
        skos:definition           "Met un item en relation avec un agent conservateur qui dresse une liste ou un inventaire des items faisant partie d’un agrégat par assemblage."@fr ;
        rdakit:toolkitLabel       "agent conservateur de collection"@fr ;
        rdakit:toolkitDefinition  "Agent conservateur qui dresse une liste ou un inventaire des items faisant partie d’un agrégat par assemblage."@fr ;
        rdakit:toolkitLabel       "conservador de colección"@es ;
        rdakit:toolkitDefinition  "Un conservador que lista o hace inventarios de ítems en una obra agregada tal como una colección de ítems u obras."@es ;
        rdakit:instructionNumber  "18.5" ;
        reg:hasSubproperty        <http://rdaregistry.info/Elements/i/object/P40005> ;
        reg:name                  "ngườiGiữBộSưuTập"@vi ;
        rdfs:label                "có người giữ bộ sưu tập"@vi ;
        skos:definition           "Liên kết bản với người giữ bộ sưu tập, người lập danh mục hoặc bản kê trong một tác phẩm gộp chung như là bộ sưu tập của các bản hoặc tác phẩm."@vi ;
        rdakit:toolkitLabel       "người giữ bộ sưu tập"@vi ;
        rdakit:toolkitDefinition  "Người giữ bộ sưu tập, người lập danh mục hoặc bản kê trong một tác phẩm gộp chung như là bộ sưu tập của các bản hoặc tác phẩm."@vi ;
        reg:name                  "samlingsregistrator"@da ;
        rdfs:label                "har samlingsregistrator"@da ;
        reg:lexicalAlias          <http://rdaregistry.info/Elements/i/samlingsregistrator.da> ;
        skos:definition           "Relaterer et eksemplar til en kurator, der har opstillet en liste eller udarbejdet en inventarliste over eksemplarer i et samlingsværk, såsom en samling af eksemplarer eller værker."@da ;
        rdakit:toolkitLabel       "samlingsregistrator"@da ;
        rdakit:toolkitDefinition  "Kurator, der har opstillet en liste eller udarbejdet en inventarliste over eksemplarer i et samlingsværk, såsom en samling af eksemplarer eller værker."@da ;
        rdfs:label                "hat Registrar"@de ;
        skos:definition           "Setzt ein Exemplar mit einem Kurator, der die Exemplare eines aggregierten Werks, wie beispielsweise eine Sammlung von Exemplaren oder Werken, verzeichnet und inventarisiert, in Beziehung."@de ;
        rdakit:toolkitLabel       "Registrar"@de ;
        rdakit:toolkitDefinition  "Ein Kurator, der die Exemplare eines aggregierten Werks, wie beispielsweise eine Sammlung von Exemplaren oder Werken, verzeichnet und inventarisiert."@de ;
        reg:name                  "υπεύθυνοςΓραμματέαςΤηςΣυλλογής"@el ;
        rdfs:label                "έχει υπεύθυνο γραμματείας της συλλογής"@el ;
        reg:lexicalAlias          <http://rdaregistry.info/Elements/i/υπεύθυνοςΓραμματέαςΤηςΣυλλογής.el> ;
        skos:definition           "Συνδέει ένα αντίτυπο με έναν έφορο ο οποίος απαριθμεί ή καταγράφει τα αντίτυπα σε ένα συγκεντρωτικό έργο, όπως μια συλλογή αντιτύπων ή έργων."@el ;
        rdakit:toolkitLabel       "υπεύθυνος γραμματείας της συλλογής"@el ;
        rdakit:toolkitDefinition  "Ένας έφορος που απαριθμεί ή καταγράφει τα αντίτυπα σε ένα συγκεντρωτικό έργο, όπως μια συλλογή αντιτύπων ή έργων."@el ;
        rdfs:label                "té com a conservador de col·leccions"@ca ;
        skos:definition           "Relaciona un item amb un conservador que llista o inventaria els ítems en una obra agregada, com ara una col·lecció d’ítems o d’obres."@ca ;
        rdakit:toolkitLabel       "conservador de col·leccions"@ca ;
        rdakit:toolkitDefinition  "Conservador que llista o inventaria els ítems en una obra agregada, com ara una col·lecció d’ítems o d’obres."@ca ;
        reg:name                  "kokoelmanLuetteloija"@fi ;
        rdfs:label                "kokoelman luetteloija"@fi ;
        reg:lexicalAlias          <rdaa:kokoelmanLuetteloija.fi> ;
        skos:definition           "Liittää kappaleen kuraattoriin, joka luetteloi tai inventoi agregaattiteokseen eli esine- tai teoskokoelmaan kuuluvat kappaleet."@fi ;
        rdakit:toolkitLabel       "kokoelman luetteloija"@fi ;
        rdakit:toolkitDefinition  "Kuraattori, joka luetteloi tai inventoi agregaattiteokseen eli esine- tai teoskokoelmaan kuuluvat kappaleet."@fi ;
        reg:name                  "conservateurDeCollection"@fr ;
        reg:lexicalAlias          <http://rdaregistry.info/Elements/i/agentConservateurDeCollection.fr> ;
        rdakit:toolkitLabel       "samlingsregistrator"@no ;
        rdakit:toolkitDefinition  "En kurator som lager lister eller oversikter over eksemplarene i et samlingsverk, for eksempel en samling av eksemplarer eller verk."@no ;
        rdakit:hasElementType     "2" ;
        reg:name                  "gyűjteményVezető"@hu ;
        rdfs:label                "van gyűjteményvezetője"@hu ;
        skos:definition           "Egy példányt hozzákapcsol egy gyűjteményvezetőhöz, aki példányokat listáz vagy leltárba vesz egy olyan összesített műben, mint egy példányok vagy művek gyűjteménye. "@hu ;
        rdakit:toolkitLabel       "gyűjteményvezető"@hu ;
        rdakit:toolkitDefinition  "Egy kurátor, aki példányokat listáz vagy leltároz egy olyan összesített műben, mint például példányok vagy művek gyűjteménye. "@hu ;
        skos:altLabel             "collection registrar"@en ;
        skos:altLabel             "conservateur de collection"@fr .

<http://rdaregistry.info/Elements/i/P40122>
        rdfs:isDefinedBy          <http://rdaregistry.info/Elements/i/> ;
        reg:status                <http://metadataregistry.org/uri/RegStatus/1001> ;
        rdfs:label                "has collection registrar collective agent"@en ;
        reg:lexicalAlias          <http://rdaregistry.info/Elements/i/collectionRegistrarCollectiveAgent.en> ;
        skos:definition           "Relates an item to a collective agent who is a curator who lists or inventories items in a collection aggregate."@en ;
        rdakit:toolkitLabel       "collection registrar collective agent"@en ;
        rdakit:toolkitDefinition  "A collective agent who is a curator who lists or inventories items in a collection aggregate."@en ;
        rdf:type                  rdf:Property ;
        reg:name                  "collectionRegistrarCollectiveAgent" ;
        rdfs:domain               <http://rdaregistry.info/Elements/c/C10003> ;
        rdakit:hasElementType     "2" ;
        reg:hasSubproperty        <http://rdaregistry.info/Elements/i/datatype/P40122> ;
        reg:hasSubproperty        <http://rdaregistry.info/Elements/i/object/P40122> ;
        rdfs:subPropertyOf        <http://rdaregistry.info/Elements/i/P40115> ;
        rdfs:subPropertyOf        <http://rdaregistry.info/Elements/i/P40005> ;
        reg:hasSubproperty        <http://rdaregistry.info/Elements/i/P40138> ;
        reg:hasSubproperty        <http://rdaregistry.info/Elements/i/P40154> ;
        reg:hasUnconstrained      <http://rdaregistry.info/Elements/u/P60067> ;
        rdfs:label                "a pour agent collectif conservateur de collection"@fr ;
        skos:definition           "Met un item en relation avec un agent collectif conservateur qui dresse une liste ou un inventaire des items faisant partie d’un agrégat par assemblage."@fr ;
        rdakit:toolkitLabel       "agent collectif conservateur de collection"@fr ;
        rdakit:toolkitDefinition  "Agent collectif conservateur qui dresse une liste ou un inventaire des items faisant partie d’un agrégat par assemblage."@fr ;
        reg:lexicalAlias          <http://rdaregistry.info/Elements/i/agentCollectifConservateurDeCollection.fr> .

<http://rdaregistry.info/Elements/i/P40138>
        rdfs:isDefinedBy          <http://rdaregistry.info/Elements/i/> ;
        reg:status                <http://metadataregistry.org/uri/RegStatus/1001> ;
        rdfs:label                "has collection registrar corporate body"@en ;
        reg:lexicalAlias          <http://rdaregistry.info/Elements/i/collectionRegistrarCorporateBody.en> ;
        skos:definition           "Relates an item to a corporate body who is a curator who lists or inventories items in a collection aggregate."@en ;
        rdakit:toolkitLabel       "collection registrar corporate body"@en ;
        rdakit:toolkitDefinition  "A corporate body who is a curator who lists or inventories items in a collection aggregate."@en ;
        rdf:type                  rdf:Property ;
        reg:name                  "collectionRegistrarCorporateBody" ;
        rdfs:domain               <http://rdaregistry.info/Elements/c/C10003> ;
        rdakit:hasElementType     "2" ;
        reg:hasSubproperty        <http://rdaregistry.info/Elements/i/datatype/P40138> ;
        reg:hasSubproperty        <http://rdaregistry.info/Elements/i/object/P40138> ;
        rdfs:subPropertyOf        <http://rdaregistry.info/Elements/i/P40131> ;
        rdfs:subPropertyOf        <http://rdaregistry.info/Elements/i/P40122> ;
        reg:hasUnconstrained      <http://rdaregistry.info/Elements/u/P60067> ;
        rdfs:label                "a pour collectivité conservatrice de collection"@fr ;
        skos:definition           "Met un item en relation avec une collectivité conservatrice qui dresse une liste ou un inventaire des items faisant partie d’un agrégat par assemblage."@fr ;
        rdakit:toolkitLabel       "collectivité conservatrice de collection"@fr ;
        rdakit:toolkitDefinition  "Collectivité conservatrice qui dresse une liste ou un inventaire des items faisant partie d’un agrégat par assemblage."@fr ;
        reg:lexicalAlias          <http://rdaregistry.info/Elements/i/collectivitéConservatriceDeCollection.fr> .

<http://rdaregistry.info/Elements/i/P40154>
        rdfs:isDefinedBy          <http://rdaregistry.info/Elements/i/> ;
        reg:status                <http://metadataregistry.org/uri/RegStatus/1001> ;
        rdfs:label                "has collection registrar family"@en ;
        reg:lexicalAlias          <http://rdaregistry.info/Elements/i/collectionRegistrarFamily.en> ;
        skos:definition           "Relates an item to a family who is a curator who lists or inventories items in a collection aggregate."@en ;
        rdakit:toolkitLabel       "collection registrar family"@en ;
        rdakit:toolkitDefinition  "A family who is a curator who lists or inventories items in a collection aggregate."@en ;
        rdf:type                  rdf:Property ;
        reg:name                  "collectionRegistrarFamily" ;
        rdfs:domain               <http://rdaregistry.info/Elements/c/C10003> ;
        rdakit:hasElementType     "2" ;
        reg:hasSubproperty        <http://rdaregistry.info/Elements/i/datatype/P40154> ;
        reg:hasSubproperty        <http://rdaregistry.info/Elements/i/object/P40154> ;
        rdfs:subPropertyOf        <http://rdaregistry.info/Elements/i/P40147> ;
        rdfs:subPropertyOf        <http://rdaregistry.info/Elements/i/P40122> ;
        reg:hasUnconstrained      <http://rdaregistry.info/Elements/u/P60067> ;
        rdfs:label                "a pour famille conservatrice de collection"@fr ;
        skos:definition           "Met un item en relation avec une famille conservatrice qui dresse une liste ou un inventaire des items faisant partie d’un agrégat par assemblage."@fr ;
        rdakit:toolkitLabel       "famille conservatrice de collection"@fr ;
        rdakit:toolkitDefinition  "Famille conservatrice qui dresse une liste ou un inventaire des items faisant partie d’un agrégat par assemblage."@fr ;
        reg:lexicalAlias          <http://rdaregistry.info/Elements/i/familleConservatriceDeCollection.fr> .

<http://rdaregistry.info/Elements/i/P40106>
        rdfs:isDefinedBy          <http://rdaregistry.info/Elements/i/> ;
        reg:status                <http://metadataregistry.org/uri/RegStatus/1001> ;
        rdfs:label                "has collection registrar person"@en ;
        reg:lexicalAlias          <http://rdaregistry.info/Elements/i/collectionRegistrarPerson.en> ;
        skos:definition           "Relates an item to a person who is a curator who lists or inventories items in a collection aggregate."@en ;
        rdakit:toolkitLabel       "collection registrar person"@en ;
        rdakit:toolkitDefinition  "A person who is a curator who lists or inventories items in a collection aggregate."@en ;
        rdf:type                  rdf:Property ;
        reg:name                  "collectionRegistrarPerson" ;
        rdfs:domain               <http://rdaregistry.info/Elements/c/C10003> ;
        rdakit:hasElementType     "2" ;
        reg:hasSubproperty        <http://rdaregistry.info/Elements/i/datatype/P40106> ;
        reg:hasSubproperty        <http://rdaregistry.info/Elements/i/object/P40106> ;
        rdfs:subPropertyOf        <http://rdaregistry.info/Elements/i/P40099> ;
        rdfs:subPropertyOf        <http://rdaregistry.info/Elements/i/P40005> ;
        reg:hasUnconstrained      <http://rdaregistry.info/Elements/u/P60067> ;
        rdfs:label                "a pour personne conservatrice de collection"@fr ;
        skos:definition           "Met un item en relation avec une personne conservatrice qui dresse une liste ou un inventaire des items faisant partie d’un agrégat par assemblage."@fr ;
        rdakit:toolkitLabel       "personne conservatrice de collection"@fr ;
        rdakit:toolkitDefinition  "Personne conservatrice qui dresse une liste ou un inventaire des items faisant partie d’un agrégat par assemblage."@fr ;
        reg:lexicalAlias          <http://rdaregistry.info/Elements/i/personneConservatriceDeCollection.fr> .

<http://rdaregistry.info/Elements/i/P40004>
        rdfs:isDefinedBy          <http://rdaregistry.info/Elements/i/> ;
        reg:status                <http://metadataregistry.org/uri/RegStatus/1001> ;
        reg:name                  "collectorAgent"@en ;
        rdfs:label                "has collector agent"@en ;
        skos:definition           "Relates an item to an agent who is a curator who brings together items from various sources that are arranged, described, or catalogued as a collection."@en ;
        rdf:type                  rdf:Property ;
        rdfs:domain               <http://rdaregistry.info/Elements/c/C10003> ;
        rdfs:subPropertyOf        <http://rdaregistry.info/Elements/i/P40017> ;
        reg:lexicalAlias          <http://rdaregistry.info/Elements/i/collectorAgent.en> ;
        reg:hasUnconstrained      <http://rdaregistry.info/Elements/u/P60066> ;
        rdakit:toolkitLabel       "collector agent"@en ;
        rdakit:toolkitDefinition  "An agent who is a curator who brings together items from various sources that are arranged, described, or catalogued as a collection."@en ;
        rdfs:label                "a pour agent collectionneur"@fr ;
        skos:definition           "Met un item en relation avec un agent conservateur qui rassemble des items de diverses sources qui sont arrangés, décrits et catalogués comme une collection."@fr ;
        rdakit:toolkitLabel       "agent collectionneur"@fr ;
        rdakit:toolkitDefinition  "Agent conservateur qui rassemble des items de diverses sources qui sont arrangés, décrits et catalogués comme une collection."@fr ;
        rdakit:toolkitLabel       "coleccionista"@es ;
        rdakit:toolkitDefinition  "Un conservador que reúne ítems de varias fuentes que luego se arreglan, describen y catalogan como una colección."@es ;
        rdakit:instructionNumber  "18.5" ;
        reg:hasSubproperty        <http://rdaregistry.info/Elements/i/object/P40004> ;
        reg:name                  "ngườiThuThập"@vi ;
        rdfs:label                "có người thu thập"@vi ;
        skos:definition           "Liên kết bản với người thu thập gop góp các bản từ các nguồn khác nhau sau đó sắp xếp, mô tả, và lập mục lục như là bộ sưu tập."@vi ;
        rdakit:toolkitLabel       "người thu thập"@vi ;
        rdakit:toolkitDefinition  "Người thu thập gop góp các bản từ các nguồn khác nhau sau đó sắp xếp, mô tả, và lập mục lục như là bộ sưu tập."@vi ;
        reg:name                  "samler"@da ;
        rdfs:label                "har samler"@da ;
        reg:lexicalAlias          <http://rdaregistry.info/Elements/i/samler.da> ;
        skos:definition           "Relaterer et eksemplar til en kurator, der har indsamlet eksemplarer fra forskellige kilder, som så er blevet arrangeret, beskrevet og katalogiseret som en samling."@da ;
        rdakit:toolkitLabel       "samler"@da ;
        rdakit:toolkitDefinition  "Kurator, der har indsamlet eksemplarer fra forskellige kilder, som er blevet arrangeret, beskrevet og katalogiseret som en samling."@da ;
        rdfs:label                "hat Sammler"@de ;
        skos:definition           "Setzt ein Exemplar mit einem Kurator, der Materialien aus unterschiedlichen Quellen zusammenträgt, die dann als Sammlung geordnet, beschrieben und katalogisiert werden, in Beziehung."@de ;
        rdakit:toolkitLabel       "Sammler"@de ;
        rdakit:toolkitDefinition  "Ein Kurator, der Materialien aus unterschiedlichen Quellen zusammenträgt, die dann als Sammlung geordnet, beschrieben und katalogisiert werden."@de ;
        reg:name                  "συλλέκτης"@el ;
        rdfs:label                "έχει συλλέκτη"@el ;
        reg:lexicalAlias          <http://rdaregistry.info/Elements/i/συλλέκτης.el> ;
        skos:definition           "Συνδέει ένα αντίτυπο με έναν έφορο που συγκεντρώνει αντίτυπα από διάφορες πηγές τα οποία κατόπιν οργανώνονται, περιγράφονται και καταλογογραφούνται ως συλλογή."@el ;
        rdakit:toolkitLabel       "συλλέκτης"@el ;
        rdakit:toolkitDefinition  "Ένας έφορος που συγκεντρώνει αντίτυπα από διάφορες πηγές, τα οποία κατόπιν οργανώνονται, περιγράφονται και καταλογογραφούνται ως συλλογή."@el ;
        rdfs:label                "té com a col·leccionista"@ca ;
        skos:definition           "Relaciona un item amb un conservador que aplega ítems de diverses fonts que posteriorment s’arrangen, es descriuen i es cataloguen com una col·lecció."@ca ;
        rdakit:toolkitLabel       "col·leccionista"@ca ;
        rdakit:toolkitDefinition  "Conservador que aplega ítems de diverses fonts que posteriorment s’arrangen, es descriuen i es cataloguen com una col·lecció."@ca ;
        reg:name                  "kokoelmanMuodostaja"@fi ;
        rdfs:label                "kokoelman muodostaja"@fi ;
        reg:lexicalAlias          <rdaa:kokoelmanMuodostaja.fi> ;
        skos:definition           "Liittää kappaleen kuraattoriin, joka kokoaa eri lähteistä kappaleita, jotka sitten järjestetään, kuvaillaan ja luetteloidaan kokoelmaksi."@fi ;
        rdakit:toolkitLabel       "kokoelman muodostaja"@fi ;
        rdakit:toolkitDefinition  "Kuraattori, joka kokoaa eri lähteistä kappaleita, jotka sitten järjestetään, kuvaillaan ja luetteloidaan kokoelmaksi."@fi ;
        reg:name                  "collectionneur"@fr ;
        reg:lexicalAlias          <http://rdaregistry.info/Elements/i/agentCollectionneur.fr> ;
        rdakit:toolkitLabel       "samler"@no ;
        rdakit:toolkitDefinition  "En kurator som kombinerer eksemplarer fra ulike kilder og deretter arrangerer, beskriver og katalogiserer dem som en samling."@no ;
        rdakit:hasElementType     "2" ;
        reg:name                  "gyűjtő"@hu ;
        rdfs:label                "van gyűjtője"@hu ;
        skos:definition           "Egy példányt hozzákapcsol egy kurátorhoz, aki különféle forrásokból példányokat hoz össze, amelyeket aztán elrendezi, leírja és gyűjteményként katalogizálja. "@hu ;
        rdakit:toolkitLabel       "gyűjtő"@hu ;
        rdakit:toolkitDefinition  "Egy kurátor, aki különféle forrásokból példányokat hoz össze, amelyeket aztán elrendeznek, leírnak és gyűjteményként katalogizálnak. "@hu ;
        skos:altLabel             "collector"@en ;
        skos:altLabel             "collectionneur"@fr .

<http://rdaregistry.info/Elements/i/P40121>
        rdfs:isDefinedBy          <http://rdaregistry.info/Elements/i/> ;
        reg:status                <http://metadataregistry.org/uri/RegStatus/1001> ;
        rdfs:label                "has collector collective agent"@en ;
        reg:lexicalAlias          <http://rdaregistry.info/Elements/i/collectorCollectiveAgent.en> ;
        skos:definition           "Relates an item to a collective agent who is a curator who brings together items from various sources that are arranged, described, or catalogued as a collection."@en ;
        rdakit:toolkitLabel       "collector collective agent"@en ;
        rdakit:toolkitDefinition  "A collective agent who is a curator who brings together items from various sources that are arranged, described, or catalogued as a collection."@en ;
        rdf:type                  rdf:Property ;
        reg:name                  "collectorCollectiveAgent" ;
        rdfs:domain               <http://rdaregistry.info/Elements/c/C10003> ;
        rdakit:hasElementType     "2" ;
        reg:hasSubproperty        <http://rdaregistry.info/Elements/i/datatype/P40121> ;
        reg:hasSubproperty        <http://rdaregistry.info/Elements/i/object/P40121> ;
        rdfs:subPropertyOf        <http://rdaregistry.info/Elements/i/P40115> ;
        rdfs:subPropertyOf        <http://rdaregistry.info/Elements/i/P40004> ;
        reg:hasSubproperty        <http://rdaregistry.info/Elements/i/P40137> ;
        reg:hasSubproperty        <http://rdaregistry.info/Elements/i/P40153> ;
        reg:hasUnconstrained      <http://rdaregistry.info/Elements/u/P60066> ;
        rdfs:label                "a pour agent collectif collectionneur"@fr ;
        skos:definition           "Met un item en relation avec un agent collectif conservateur qui rassemble des items de diverses sources qui sont arrangés, décrits et catalogués comme une collection."@fr ;
        rdakit:toolkitLabel       "agent collectif collectionneur"@fr ;
        rdakit:toolkitDefinition  "Agent collectif conservateur qui rassemble des items de diverses sources qui sont arrangés, décrits et catalogués comme une collection."@fr ;
        reg:lexicalAlias          <http://rdaregistry.info/Elements/i/agentCollectifCollectionneur.fr> .

<http://rdaregistry.info/Elements/i/P40137>
        rdfs:isDefinedBy          <http://rdaregistry.info/Elements/i/> ;
        reg:status                <http://metadataregistry.org/uri/RegStatus/1001> ;
        rdfs:label                "has collector corporate body"@en ;
        reg:lexicalAlias          <http://rdaregistry.info/Elements/i/collectorCorporateBody.en> ;
        skos:definition           "Relates an item to a corporate body who is a curator who brings together items from various sources that are arranged, described, or catalogued as a collection."@en ;
        rdakit:toolkitLabel       "collector corporate body"@en ;
        rdakit:toolkitDefinition  "A corporate body who is a curator who brings together items from various sources that are arranged, described, or catalogued as a collection."@en ;
        rdf:type                  rdf:Property ;
        reg:name                  "collectorCorporateBody" ;
        rdfs:domain               <http://rdaregistry.info/Elements/c/C10003> ;
        rdakit:hasElementType     "2" ;
        reg:hasSubproperty        <http://rdaregistry.info/Elements/i/datatype/P40137> ;
        reg:hasSubproperty        <http://rdaregistry.info/Elements/i/object/P40137> ;
        rdfs:subPropertyOf        <http://rdaregistry.info/Elements/i/P40131> ;
        rdfs:subPropertyOf        <http://rdaregistry.info/Elements/i/P40121> ;
        reg:hasUnconstrained      <http://rdaregistry.info/Elements/u/P60066> ;
        rdfs:label                "a pour collectivité collectionneuse"@fr ;
        skos:definition           "Met un item en relation avec une collectivité conservatrice qui rassemble des items de diverses sources qui sont arrangés, décrits et catalogués comme une collection."@fr ;
        rdakit:toolkitLabel       "collectivité collectionneuse"@fr ;
        rdakit:toolkitDefinition  "Collectivité conservatrice qui rassemble des items de diverses sources qui sont arrangés, décrits et catalogués comme une collection."@fr ;
        reg:lexicalAlias          <http://rdaregistry.info/Elements/i/collectivitéCollectionneuse.fr> .

<http://rdaregistry.info/Elements/i/P40153>
        rdfs:isDefinedBy          <http://rdaregistry.info/Elements/i/> ;
        reg:status                <http://metadataregistry.org/uri/RegStatus/1001> ;
        rdfs:label                "has collector family"@en ;
        reg:lexicalAlias          <http://rdaregistry.info/Elements/i/collectorFamily.en> ;
        skos:definition           "Relates an item to a family who is a curator who brings together items from various sources that are arranged, described, or catalogued as a collection."@en ;
        rdakit:toolkitLabel       "collector family"@en ;
        rdakit:toolkitDefinition  "A family who is a curator who brings together items from various sources that are arranged, described, or catalogued as a collection."@en ;
        rdf:type                  rdf:Property ;
        reg:name                  "collectorFamily" ;
        rdfs:domain               <http://rdaregistry.info/Elements/c/C10003> ;
        rdakit:hasElementType     "2" ;
        reg:hasSubproperty        <http://rdaregistry.info/Elements/i/datatype/P40153> ;
        reg:hasSubproperty        <http://rdaregistry.info/Elements/i/object/P40153> ;
        rdfs:subPropertyOf        <http://rdaregistry.info/Elements/i/P40147> ;
        rdfs:subPropertyOf        <http://rdaregistry.info/Elements/i/P40121> ;
        reg:hasUnconstrained      <http://rdaregistry.info/Elements/u/P60066> ;
        rdfs:label                "a pour famille collectionneuse"@fr ;
        skos:definition           "Met un item en relation avec une famille conservatrice qui rassemble des items de diverses sources qui sont arrangés, décrits et catalogués comme une collection."@fr ;
        rdakit:toolkitLabel       "famille collectionneuse"@fr ;
        rdakit:toolkitDefinition  "Famille conservatrice qui rassemble des items de diverses sources qui sont arrangés, décrits et catalogués comme une collection."@fr ;
        reg:lexicalAlias          <http://rdaregistry.info/Elements/i/familleCollectionneuse.fr> .

<http://rdaregistry.info/Elements/i/P40105>
        rdfs:isDefinedBy          <http://rdaregistry.info/Elements/i/> ;
        reg:status                <http://metadataregistry.org/uri/RegStatus/1001> ;
        rdfs:label                "has collector person"@en ;
        reg:lexicalAlias          <http://rdaregistry.info/Elements/i/collectorPerson.en> ;
        skos:definition           "Relates an item to a person who is a curator who brings together items from various sources that are arranged, described, or catalogued as a collection."@en ;
        rdakit:toolkitLabel       "collector person"@en ;
        rdakit:toolkitDefinition  "A person who is a curator who brings together items from various sources that are arranged, described, or catalogued as a collection."@en ;
        rdf:type                  rdf:Property ;
        reg:name                  "collectorPerson" ;
        rdfs:domain               <http://rdaregistry.info/Elements/c/C10003> ;
        rdakit:hasElementType     "2" ;
        reg:hasSubproperty        <http://rdaregistry.info/Elements/i/datatype/P40105> ;
        reg:hasSubproperty        <http://rdaregistry.info/Elements/i/object/P40105> ;
        rdfs:subPropertyOf        <http://rdaregistry.info/Elements/i/P40099> ;
        rdfs:subPropertyOf        <http://rdaregistry.info/Elements/i/P40004> ;
        reg:hasUnconstrained      <http://rdaregistry.info/Elements/u/P60066> ;
        rdfs:label                "a pour personne collectionneuse"@fr ;
        skos:definition           "Met un item en relation avec une personne conservatrice qui rassemble des items de diverses sources qui sont arrangés, décrits et catalogués comme une collection."@fr ;
        rdakit:toolkitLabel       "personne collectionneuse"@fr ;
        rdakit:toolkitDefinition  "Personne conservatrice qui rassemble des items de diverses sources qui sont arrangés, décrits et catalogués comme une collection."@fr ;
        reg:lexicalAlias          <http://rdaregistry.info/Elements/i/personneCollectionneuse.fr> .

<http://rdaregistry.info/Elements/i/P40043>
        rdfs:isDefinedBy    <http://rdaregistry.info/Elements/i/> ;
        reg:status          <http://metadataregistry.org/uri/RegStatus/1008> ;
        rdf:type            rdf:Property ;
        rdfs:subPropertyOf  <http://rdaregistry.info/Elements/i/P40030> .

<http://rdaregistry.info/Elements/i/P40009>
        rdfs:isDefinedBy          <http://rdaregistry.info/Elements/i/> ;
        reg:status                <http://metadataregistry.org/uri/RegStatus/1001> ;
        reg:name                  "containedInItem"@en ;
        rdfs:label                "is contained in item"@en ;
        skos:definition           "Relates an item to a larger item of which an item is a discrete component."@en ;
        rdf:type                  rdf:Property ;
        rdfs:domain               <http://rdaregistry.info/Elements/c/C10003> ;
        rdfs:subPropertyOf        <http://rdaregistry.info/Elements/i/P40046> ;
        reg:lexicalAlias          <http://rdaregistry.info/Elements/i/containedInItem.en> ;
        reg:hasUnconstrained      <http://rdaregistry.info/Elements/u/P60101> ;
        rdakit:toolkitLabel       "contained in item"@en ;
        rdakit:toolkitDefinition  "A larger item of which an item is a discrete component."@en ;
        rdfs:label                "est contenu dans un item"@fr ;
        skos:definition           "Met un item en relation avec un item plus vaste dont un item est une composante distincte."@fr ;
        rdakit:toolkitLabel       "contenu dans un item"@fr ;
        rdakit:toolkitDefinition  "Item plus vaste dont un item est une composante distincte."@fr ;
        rdakit:toolkitLabel       "contenido en (ítem)"@es ;
        rdakit:toolkitDefinition  "Un ítem mayor del cual una parte es un componente separado."@es ;
        rdakit:instructionNumber  "24.5" ;
        reg:hasSubproperty        <http://rdaregistry.info/Elements/i/object/P40009> ;
        reg:name                  "đượcChứaTrongBản"@vi ;
        rdfs:label                "được chứa trong (bản)"@vi ;
        skos:definition           "Liên kết bản với bản lớn hơn trong đó một bản là một bộ phần cấu thành tách biệt."@vi ;
        rdakit:toolkitLabel       "được chứa trong (bản)"@vi ;
        rdakit:toolkitDefinition  "Bản lớn hơn trong đó một bản là một bộ phần cấu thành tách biệt."@vi ;
        reg:name                  "indeholdtIEksemplar"@da ;
        rdfs:label                "er indeholdt i (eksemplar)"@da ;
        reg:lexicalAlias          <http://rdaregistry.info/Elements/i/indeholdtIEksemplar.da> ;
        skos:definition           "Relaterer et eksemplar til et større eksemplar, som eksemplaret udgør en separat del af."@da ;
        rdakit:toolkitLabel       "indeholdt i (eksemplar)"@da ;
        rdakit:toolkitDefinition  "Større eksemplar, som eksemplaret udgør en separat del af."@da ;
        rdfs:label                "ist enthalten in (Exemplar)"@de ;
        skos:definition           "Setzt ein Exemplar mit einem größeren Exemplar, von dem ein Exemplar ein eigenständiger Bestandteil ist, in Beziehung."@de ;
        rdakit:toolkitLabel       "Enthalten in (Exemplar)"@de ;
        rdakit:toolkitDefinition  "Ein größeres Exemplar, von dem ein Exemplar ein eigenständiger Bestandteil ist."@de ;
        reg:name                  "περιέχεταιΣτοΑντίτυπο"@el ;
        rdfs:label                "περιέχεται σε (αντίτυπο)"@el ;
        reg:lexicalAlias          <http://rdaregistry.info/Elements/i/περιέχεταιΣτοΑντίτυπο.el> ;
        skos:definition           "Συνδέει ένα αντίτυπο με ένα μεγαλύτερο αντίτυπο του οποίου ένα αντίτυπο συνιστά διακριτό συστατικό."@el ;
        rdakit:toolkitLabel       "περιέχεται σε (αντίτυπο)"@el ;
        rdakit:toolkitDefinition  "Ένα μεγαλύτερο αντίτυπο του οποίου ένα αντίτυπο συνιστά διακριτό συστατικό."@el ;
        rdfs:label                "és contingut en (ítem)"@ca ;
        skos:definition           "Relaciona un item amb un ítem més ampli del qual un ítem és un component discret."@ca ;
        rdakit:toolkitLabel       "contingut en (ítem)"@ca ;
        rdakit:toolkitDefinition  "Ítem més ampli del qual un ítem és un component discret."@ca ;
        reg:name                  "sisaltyyKappaleeseen"@fi ;
        rdfs:label                "sisältyy kappaleeseen"@fi ;
        reg:lexicalAlias          <rdaa:sisaltyyKappaleeseen.fi> ;
        skos:definition           "Liittää kappaleen laajempaan kappaleseen, jonka itsenäinen osa kappale on."@fi ;
        rdakit:toolkitLabel       "sisältyy kappaleeseen"@fi ;
        rdakit:toolkitDefinition  "Laajempi kappale, jonka itsenäinen osa kappale on."@fi ;
        reg:name                  "contenuDansItem"@fr ;
        reg:lexicalAlias          <http://rdaregistry.info/Elements/i/contenuDansUnItem.fr> ;
        rdakit:toolkitLabel       "omfattes av (eksemplar)"@no ;
        rdakit:toolkitDefinition  "Et større eksemplar der et eksemplar er en avgrenset bestanddel."@no ;
        rdakit:hasElementType     "2" ;
        reg:name                  "Példánytartalmaz"@hu ;
        rdfs:label                "tartalmaz (példány)"@hu ;
        skos:definition           "Egy példányt hozzákapcsol egy nagyobb példányhoz, amelynek egy példánya különálló alkotóelem. "@hu ;
        rdakit:toolkitLabel       "tartalmaz (példány)"@hu ;
        rdakit:toolkitDefinition  "Egy nagyobb példány, amelynek egy példány a különálló alkotóeleme. "@hu .

<http://rdaregistry.info/Elements/i/P40034>
        rdfs:isDefinedBy          <http://rdaregistry.info/Elements/i/> ;
        reg:status                <http://metadataregistry.org/uri/RegStatus/1001> ;
        reg:name                  "containerOfItem"@en ;
        rdfs:label                "is container of item"@en ;
        skos:definition           "Relates an item to an item that is a discrete component of a larger item."@en ;
        rdf:type                  rdf:Property ;
        rdfs:domain               <http://rdaregistry.info/Elements/c/C10003> ;
        rdfs:subPropertyOf        <http://rdaregistry.info/Elements/i/P40046> ;
        reg:lexicalAlias          <http://rdaregistry.info/Elements/i/containerOfItem.en> ;
        reg:hasUnconstrained      <http://rdaregistry.info/Elements/u/P60249> ;
        rdakit:toolkitLabel       "container of item"@en ;
        rdakit:toolkitDefinition  "An item that is a discrete component of a larger item."@en ;
        rdfs:label                "est un conteneur d’un item"@fr ;
        skos:definition           "Met un item en relation avec un item qui est une composante distincte d’un item plus vaste."@fr ;
        rdakit:toolkitLabel       "conteneur d’un item"@fr ;
        rdakit:toolkitDefinition  "Item qui est une composante distincte d’un item plus vaste."@fr ;
        rdakit:toolkitLabel       "contiene (ítem)"@es ;
        rdakit:toolkitDefinition  "Un ítem que es un componente separado de un ítem mayor."@es ;
        rdakit:instructionNumber  "24.5" ;
        reg:hasSubproperty        <http://rdaregistry.info/Elements/i/object/P40034> ;
        reg:name                  "vỏChứaCủaBản"@vi ;
        rdfs:label                "là vỏ chứa của (bản)"@vi ;
        skos:definition           "Liên kết bản với bản là bộ phận cấu thành tách biệt của bản lớn hơn."@vi ;
        rdakit:toolkitLabel       "vỏ chứa của (bản)"@vi ;
        rdakit:toolkitDefinition  "Bản là bộ phận cấu thành tách biệt của bản lớn hơn."@vi ;
        reg:name                  "indeholderAfEksemplar"@da ;
        rdfs:label                "er indeholder af (eksemplar)"@da ;
        reg:lexicalAlias          <http://rdaregistry.info/Elements/i/indeholderAfEksemplar.da> ;
        skos:definition           "Relaterer et eksemplar til et eksemplar, der udgør en separat del af et større eksemplar."@da ;
        rdakit:toolkitLabel       "indeholder af (eksemplar)"@da ;
        rdakit:toolkitDefinition  "Eksemplar, der udgør en separat del af et større eksemplar."@da ;
        skos:definition           "Setzt ein Exemplar mit einem Exemplar, das ein eigenständiger Bestandteil eines größeren Exemplars ist, in Beziehung."@de ;
        rdakit:toolkitLabel       "Enthält (Exemplar)"@de ;
        rdakit:toolkitDefinition  "Ein Exemplar, das ein eigenständiger Bestandteil eines größeren Exemplars ist."@de ;
        reg:name                  "περιέκτηςΤουΑντιτύπου"@el ;
        rdfs:label                "είναι περιέκτης του (αντίτυπο)"@el ;
        reg:lexicalAlias          <http://rdaregistry.info/Elements/i/περιέκτηςΤουΑντιτύπου.el> ;
        skos:definition           "Συνδέει ένα αντίτυπο με ένα αντίτυπο το οποίο είναι διακριτό συστατικό ενός μεγαλύτερου αντιτύπου."@el ;
        rdakit:toolkitLabel       "περιέκτης του (αντίτυπο)"@el ;
        rdakit:toolkitDefinition  "Ένα αντίτυπο το οποίο είναι διακριτό συστατικό ενός μεγαλύτερου αντιτύπου."@el ;
        rdfs:label                "és contenidor de (ítem)"@ca ;
        skos:definition           "Relaciona un item amb un ítem que és un component discret d’un ítem més ampli."@ca ;
        rdakit:toolkitLabel       "contenidor de (ítem)"@ca ;
        rdakit:toolkitDefinition  "Ítem que és un component discret d’un ítem més ampli."@ca ;
        reg:name                  "sisaltaaKappaleen"@fi ;
        rdfs:label                "sisältää kappaleen"@fi ;
        reg:lexicalAlias          <rdaa:sisaltaaKappaleen.fi> ;
        skos:definition           "Liittää kappaleen kappaleeseen, joka on itsenäinen osa laajempaa kappaletta."@fi ;
        rdakit:toolkitLabel       "sisältää kappaleen"@fi ;
        rdakit:toolkitDefinition  "Kappale, joka on itsenäinen osa laajempaa kappaletta."@fi ;
        reg:name                  "conteneurDeItem"@fr ;
        reg:lexicalAlias          <http://rdaregistry.info/Elements/i/conteneurDunItem.fr> ;
        rdakit:toolkitLabel       "omfatter (eksemplar)"@no ;
        rdakit:toolkitDefinition  "Et eksemplar som er en avgrenset bestanddel av et større eksemplar."@no ;
        rdakit:hasElementType     "2" ;
        reg:name                  "Példánytárolója"@hu ;
        rdfs:label                "tartalmaz (példány)"@hu ;
        skos:definition           "Egy példányt hozzákapcsol egy olyan példányhoz, amely egy nagyobb példány különálló alkotóeleme."@hu ;
        rdakit:toolkitLabel       "tartója (példány)"@hu ;
        rdakit:toolkitDefinition  "Egy példány, amely egy nagyobb példány különálló alkotóeleme."@hu .

<http://rdaregistry.info/Elements/i/P40041>
        rdfs:isDefinedBy    <http://rdaregistry.info/Elements/i/> ;
        reg:status          <http://metadataregistry.org/uri/RegStatus/1008> ;
        rdf:type            rdf:Property ;
        rdfs:subPropertyOf  <http://rdaregistry.info/Elements/i/P40030> .

<http://rdaregistry.info/Elements/i/P40017>
        rdfs:isDefinedBy          <http://rdaregistry.info/Elements/i/> ;
        reg:status                <http://metadataregistry.org/uri/RegStatus/1001> ;
        reg:name                  "curatorAgent"@en ;
        rdfs:label                "has curator agent"@en ;
        skos:definition           "Relates an item to an agent who conceives or manages the aggregation of an item in an exhibition or collection."@en ;
        rdf:type                  rdf:Property ;
        rdfs:domain               <http://rdaregistry.info/Elements/c/C10003> ;
        rdfs:subPropertyOf        <http://rdaregistry.info/Elements/i/P40072> ;
        reg:hasSubproperty        <http://rdaregistry.info/Elements/i/P40004> ;
        reg:hasSubproperty        <http://rdaregistry.info/Elements/i/P40005> ;
        reg:lexicalAlias          <http://rdaregistry.info/Elements/i/curatorAgent.en> ;
        reg:hasUnconstrained      <http://rdaregistry.info/Elements/u/P60376> ;
        rdakit:toolkitLabel       "curator agent"@en ;
        rdakit:toolkitDefinition  "An agent who conceives or manages the aggregation of an item in an exhibition or collection."@en ;
        rdfs:label                "a pour agent conservateur"@fr ;
        skos:definition           "Met un item en relation avec un agent qui conçoit ou gère l’agrégation d’un item dans une exposition ou une collection."@fr ;
        rdakit:toolkitLabel       "agent conservateur"@fr ;
        rdakit:toolkitDefinition  "Agent qui conçoit ou gère l’agrégation d’un item dans une exposition ou une collection."@fr ;
        rdakit:toolkitLabel       "curador"@es ;
        rdakit:toolkitDefinition  "Una persona, familia o entidad corporativa que concibe, agrega y/o organiza una exhibición, colección u otro ítem."@es ;
        rdakit:instructionNumber  "18.5" ;
        reg:hasSubproperty        <http://rdaregistry.info/Elements/i/object/P40017> ;
        reg:name                  "ngườiTrôngNom"@vi ;
        rdfs:label                "có người trông nom"@vi ;
        skos:definition           "Liên kết bản với tác nhân tạo lập, tập hợp, hoặc tổ chức triển lãm, bộ sưu tập, hoặc hạng mục khác."@vi ;
        rdakit:toolkitLabel       "người trông nom"@vi ;
        rdakit:toolkitDefinition  "Tác nhân tạo lập, tập hợp, hoặc tổ chức triển lãm, bộ sưu tập, hoặc hạng mục khác."@vi ;
        reg:name                  "kurator"@da ;
        rdfs:label                "har kurator"@da ;
        reg:lexicalAlias          <http://rdaregistry.info/Elements/i/kurator.da> ;
        skos:definition           "Relaterer et eksemplar til en agent, der har udtænkt, samlet eller arrangeret en udstilling, samling eller andet eksemplar."@da ;
        rdakit:toolkitLabel       "kurator"@da ;
        rdakit:toolkitDefinition  "Agent, der har udtænkt, samlet eller arrangeret en udstilling, samling eller andet eksemplar."@da ;
        rdfs:label                "hat Kurator"@de ;
        skos:definition           "Setzt ein Exemplar mit einem Akteur, der eine Ausstellung, eine Sammlung oder weitere Exemplare konzipiert, zusammenstellt oder organisiert, in Beziehung."@de ;
        rdakit:toolkitLabel       "Kurator"@de ;
        rdakit:toolkitDefinition  "Ein Akteur, der eine Ausstellung, eine Sammlung oder weitere Exemplare konzipiert, zusammenstellt oder organisiert."@de ;
        reg:name                  "έφορος"@el ;
        rdfs:label                "έχει έφορο"@el ;
        reg:lexicalAlias          <http://rdaregistry.info/Elements/i/έφορος.el> ;
        skos:definition           "Συνδέει ένα αντίτυπο με έναν φορέα που συλλαμβάνει, συγκεντρώνει ή και οργανώνει μια έκθεση, συλλογή ή άλλο αντίτυπο."@el ;
        rdakit:toolkitLabel       "έφορος"@el ;
        rdakit:toolkitDefinition  "Ένας φορέας που συλλαμβάνει, συγκεντρώνει ή και οργανώνει μια έκθεση, συλλογή ή άλλο αντίτυπο."@el ;
        rdfs:label                "té com a conservador"@ca ;
        skos:definition           "Relaciona un item amb un agent que concep, aplega o organitza una exposició, una col·lecció o qualsevol altre ítem."@ca ;
        rdakit:toolkitLabel       "conservador"@ca ;
        rdakit:toolkitDefinition  "Agent que concep, aplega o organitza una exposició, una col·lecció o qualsevol altre ítem."@ca ;
        reg:name                  "kuraattori"@fi ;
        rdfs:label                "kuraattori"@fi ;
        reg:lexicalAlias          <rdaa:kuraattori.fi> ;
        skos:definition           "Liittää kappaleen toimijaan, joka on suunnitellut, koonnut ja/tai järjestänyt näyttelyn, kokoelman tms."@fi ;
        rdakit:toolkitLabel       "kuraattori"@fi ;
        rdakit:toolkitDefinition  "Toimija, joka on suunnitellut, koonnut tai järjestänyt näyttelyn, kokoelman tms."@fi ;
        reg:name                  "conservateur"@fr ;
        reg:lexicalAlias          <http://rdaregistry.info/Elements/i/agentConservateur.fr> ;
        rdakit:toolkitLabel       "kurator"@no ;
        rdakit:toolkitDefinition  "En agent som har ideen til, samler eller organiserer en utstilling, en samling eller et annet eksemplar."@no ;
        rdakit:hasElementType     "2" ;
        reg:name                  "kurátor"@hu ;
        rdfs:label                "van kurátora"@hu ;
        skos:definition           "Egy példányt hozzákapcsol egy ágenshez (személyhez, családhoz vagy testülethez), aki/amely kigondol, összegyűjt vagy megszervez egy kiállítást, gyűjteményt vagy más példányt."@hu ;
        rdakit:toolkitLabel       "kurátor"@hu ;
        rdakit:toolkitDefinition  "Egy ágens (személy, család vagy testület), aki/amely kigondol, összegyűjt vagy megszervez egy kiállítást, gyűjteményt vagy valamilyen más példányt. "@hu ;
        reg:hasSubproperty        <http://rdaregistry.info/Elements/i/datatype/P40017> ;
        skos:altLabel             "curator"@en ;
        reg:hasSubproperty        <http://rdaregistry.info/Elements/i/P40105> ;
        reg:hasSubproperty        <http://rdaregistry.info/Elements/i/P40106> ;
        reg:hasSubproperty        <http://rdaregistry.info/Elements/i/P40121> ;
        reg:hasSubproperty        <http://rdaregistry.info/Elements/i/P40122> ;
        skos:altLabel             "conservateur"@fr .

<http://rdaregistry.info/Elements/i/P40115>
        rdfs:isDefinedBy          <http://rdaregistry.info/Elements/i/> ;
        reg:status                <http://metadataregistry.org/uri/RegStatus/1001> ;
        rdfs:label                "has curator collective agent"@en ;
        reg:lexicalAlias          <http://rdaregistry.info/Elements/i/curatorCollectiveAgent.en> ;
        skos:definition           "Relates an item to a collective agent who conceives or manages the aggregation of an item in an exhibition or collection."@en ;
        rdakit:toolkitLabel       "curator collective agent"@en ;
        rdakit:toolkitDefinition  "A collective agent who conceives or manages the aggregation of an item in an exhibition or collection."@en ;
        rdf:type                  rdf:Property ;
        reg:name                  "curatorCollectiveAgent" ;
        rdfs:domain               <http://rdaregistry.info/Elements/c/C10003> ;
        rdakit:hasElementType     "2" ;
        reg:hasSubproperty        <http://rdaregistry.info/Elements/i/datatype/P40115> ;
        reg:hasSubproperty        <http://rdaregistry.info/Elements/i/object/P40115> ;
        rdfs:subPropertyOf        <http://rdaregistry.info/Elements/i/P40076> ;
        rdfs:subPropertyOf        <http://rdaregistry.info/Elements/i/P40017> ;
        reg:hasSubproperty        <http://rdaregistry.info/Elements/i/P40121> ;
        reg:hasSubproperty        <http://rdaregistry.info/Elements/i/P40122> ;
        reg:hasSubproperty        <http://rdaregistry.info/Elements/i/P40131> ;
        reg:hasSubproperty        <http://rdaregistry.info/Elements/i/P40147> ;
        reg:hasUnconstrained      <http://rdaregistry.info/Elements/u/P60376> ;
        rdfs:label                "a pour agent collectif conservateur"@fr ;
        skos:definition           "Met un item en relation avec un agent collectif qui conçoit ou gère l’agrégation d’un item dans une exposition ou une collection."@fr ;
        rdakit:toolkitLabel       "agent collectif conservateur"@fr ;
        rdakit:toolkitDefinition  "Agent collectif qui conçoit ou gère l’agrégation d’un item dans une exposition ou une collection."@fr ;
        reg:lexicalAlias          <http://rdaregistry.info/Elements/i/agentCollectifConservateur.fr> .

<http://rdaregistry.info/Elements/i/P40131>
        rdfs:isDefinedBy          <http://rdaregistry.info/Elements/i/> ;
        reg:status                <http://metadataregistry.org/uri/RegStatus/1001> ;
        rdfs:label                "has curator corporate body"@en ;
        reg:lexicalAlias          <http://rdaregistry.info/Elements/i/curatorCorporateBody.en> ;
        skos:definition           "Relates an item to a corporate body who conceives or manages the aggregation of an item in an exhibition or collection."@en ;
        rdakit:toolkitLabel       "curator corporate body"@en ;
        rdakit:toolkitDefinition  "A corporate body who conceives or manages the aggregation of an item in an exhibition or collection."@en ;
        rdf:type                  rdf:Property ;
        reg:name                  "curatorCorporateBody" ;
        rdfs:domain               <http://rdaregistry.info/Elements/c/C10003> ;
        rdakit:hasElementType     "2" ;
        reg:hasSubproperty        <http://rdaregistry.info/Elements/i/datatype/P40131> ;
        reg:hasSubproperty        <http://rdaregistry.info/Elements/i/object/P40131> ;
        rdfs:subPropertyOf        <http://rdaregistry.info/Elements/i/P40075> ;
        rdfs:subPropertyOf        <http://rdaregistry.info/Elements/i/P40115> ;
        reg:hasSubproperty        <http://rdaregistry.info/Elements/i/P40137> ;
        reg:hasSubproperty        <http://rdaregistry.info/Elements/i/P40138> ;
        reg:hasUnconstrained      <http://rdaregistry.info/Elements/u/P60376> ;
        rdfs:label                "a pour collectivité conservatrice"@fr ;
        skos:definition           "Met un item en relation avec une collectivité qui conçoit ou gère l’agrégation d’un item dans une exposition ou une collection."@fr ;
        rdakit:toolkitLabel       "collectivité conservatrice"@fr ;
        rdakit:toolkitDefinition  "Collectivité qui conçoit ou gère l’agrégation d’un item dans une exposition ou une collection."@fr ;
        reg:lexicalAlias          <http://rdaregistry.info/Elements/i/collectivitéConservatrice.fr> .

<http://rdaregistry.info/Elements/i/P40147>
        rdfs:isDefinedBy          <http://rdaregistry.info/Elements/i/> ;
        reg:status                <http://metadataregistry.org/uri/RegStatus/1001> ;
        rdfs:label                "has curator family"@en ;
        reg:lexicalAlias          <http://rdaregistry.info/Elements/i/curatorFamily.en> ;
        skos:definition           "Relates an item to a family who conceives or manages the aggregation of an item in an exhibition or collection."@en ;
        rdakit:toolkitLabel       "curator family"@en ;
        rdakit:toolkitDefinition  "A family who conceives or manages the aggregation of an item in an exhibition or collection."@en ;
        rdf:type                  rdf:Property ;
        reg:name                  "curatorFamily" ;
        rdfs:domain               <http://rdaregistry.info/Elements/c/C10003> ;
        rdakit:hasElementType     "2" ;
        reg:hasSubproperty        <http://rdaregistry.info/Elements/i/datatype/P40147> ;
        reg:hasSubproperty        <http://rdaregistry.info/Elements/i/object/P40147> ;
        rdfs:subPropertyOf        <http://rdaregistry.info/Elements/i/P40074> ;
        rdfs:subPropertyOf        <http://rdaregistry.info/Elements/i/P40115> ;
        reg:hasSubproperty        <http://rdaregistry.info/Elements/i/P40153> ;
        reg:hasSubproperty        <http://rdaregistry.info/Elements/i/P40154> ;
        reg:hasUnconstrained      <http://rdaregistry.info/Elements/u/P60376> ;
        rdfs:label                "a pour famille conservatrice"@fr ;
        skos:definition           "Met un item en relation avec une famille qui conçoit ou gère l’agrégation d’un item dans une exposition ou une collection."@fr ;
        rdakit:toolkitLabel       "famille conservatrice"@fr ;
        rdakit:toolkitDefinition  "Famille qui conçoit ou gère l’agrégation d’un item dans une exposition ou une collection."@fr ;
        reg:lexicalAlias          <http://rdaregistry.info/Elements/i/familleConservatrice.fr> .

<http://rdaregistry.info/Elements/i/P40099>
        rdfs:isDefinedBy          <http://rdaregistry.info/Elements/i/> ;
        reg:status                <http://metadataregistry.org/uri/RegStatus/1001> ;
        rdfs:label                "has curator person"@en ;
        reg:lexicalAlias          <http://rdaregistry.info/Elements/i/curatorPerson.en> ;
        skos:definition           "Relates an item to a person who conceives or manages the aggregation of an item in an exhibition or collection."@en ;
        rdakit:toolkitLabel       "curator person"@en ;
        rdakit:toolkitDefinition  "A person who conceives or manages the aggregation of an item in an exhibition or collection."@en ;
        rdf:type                  rdf:Property ;
        reg:name                  "curatorPerson" ;
        rdfs:domain               <http://rdaregistry.info/Elements/c/C10003> ;
        rdakit:hasElementType     "2" ;
        reg:hasSubproperty        <http://rdaregistry.info/Elements/i/datatype/P40099> ;
        reg:hasSubproperty        <http://rdaregistry.info/Elements/i/object/P40099> ;
        rdfs:subPropertyOf        <http://rdaregistry.info/Elements/i/P40073> ;
        rdfs:subPropertyOf        <http://rdaregistry.info/Elements/i/P40017> ;
        reg:hasSubproperty        <http://rdaregistry.info/Elements/i/P40105> ;
        reg:hasSubproperty        <http://rdaregistry.info/Elements/i/P40106> ;
        reg:hasUnconstrained      <http://rdaregistry.info/Elements/u/P60376> ;
        rdfs:label                "a pour personne conservatrice"@fr ;
        skos:definition           "Met un item en relation avec une personne qui conçoit ou gère l’agrégation d’un item dans une exposition ou une collection."@fr ;
        rdakit:toolkitLabel       "personne conservatrice"@fr ;
        rdakit:toolkitDefinition  "Personne qui conçoit ou gère l’agrégation d’un item dans une exposition ou une collection."@fr ;
        reg:lexicalAlias          <http://rdaregistry.info/Elements/i/personneConservatrice.fr> .

<http://rdaregistry.info/Elements/i/P40018>
        rdfs:isDefinedBy          <http://rdaregistry.info/Elements/i/> ;
        reg:status                <http://metadataregistry.org/uri/RegStatus/1001> ;
        reg:name                  "currentOwnerAgent"@en ;
        rdfs:label                "has current owner agent"@en ;
        skos:definition           "Relates an item to an agent who has current legal possession of an item."@en ;
        rdf:type                  rdf:Property ;
        rdfs:domain               <http://rdaregistry.info/Elements/c/C10003> ;
        rdfs:subPropertyOf        <http://rdaregistry.info/Elements/i/P40021> ;
        reg:hasSubproperty        <http://rdaregistry.info/Elements/i/P40006> ;
        reg:lexicalAlias          <http://rdaregistry.info/Elements/i/currentOwnerAgent.en> ;
        reg:hasUnconstrained      <http://rdaregistry.info/Elements/u/P60400> ;
        rdakit:toolkitLabel       "current owner agent"@en ;
        rdakit:toolkitDefinition  "An agent who has current legal possession of an item."@en ;
        rdfs:label                "a pour agent propriétaire actuel"@fr ;
        skos:definition           "Met un item en relation avec un agent qui possède actuellement et légalement un item."@fr ;
        rdakit:toolkitLabel       "agent propriétaire actuel"@fr ;
        rdakit:toolkitDefinition  "Agent qui possède actuellement et légalement un item."@fr ;
        rdakit:toolkitLabel       "propietario actual"@es ;
        rdakit:toolkitDefinition  "Una persona, familia o entidad corporativa que actualmente tiene la posesión legal de un ítem."@es ;
        rdakit:instructionNumber  "18.5" ;
        reg:hasSubproperty        <http://rdaregistry.info/Elements/i/object/P40018> ;
        reg:name                  "ngườiChủHiệnTại"@vi ;
        rdfs:label                "có người chủ hiện tại"@vi ;
        skos:definition           "Liên kết bản với tác nhân hiện đang sở hữu theo pháp luật một bản."@vi ;
        rdakit:toolkitLabel       "người chủ hiện tại"@vi ;
        rdakit:toolkitDefinition  "Tác nhân hiện đang sở hữu theo pháp luật một bản."@vi ;
        reg:name                  "nuværendeEjer"@da ;
        rdfs:label                "har nuværende ejer"@da ;
        reg:lexicalAlias          <http://rdaregistry.info/Elements/i/nuværendeEjer.da> ;
        skos:definition           "Relaterer et eksemplar til en agent, der p.t. er i lovlig besiddelse af et eksemplar."@da ;
        rdakit:toolkitLabel       "nuværende ejer"@da ;
        rdakit:toolkitDefinition  "Agent, der p.t. er i lovlig besiddelse af et eksemplar."@da ;
        rdfs:label                "hat gegenwärtigen Eigentümer"@de ;
        skos:definition           "Setzt ein Exemplar mit einem Akteur, der derzeit im rechtmäßigen Besitz eines Exemplars ist, in Beziehung."@de ;
        rdakit:toolkitLabel       "Gegenwärtiger Eigentümer"@de ;
        rdakit:toolkitDefinition  "Ein Akteur, der derzeit im rechtmäßigen Besitz eines Exemplars ist."@de ;
        reg:name                  "τρέχωνΙδιοκτήτης"@el ;
        rdfs:label                "έχει τρέχοντα ιδιοκτήτη"@el ;
        reg:lexicalAlias          <http://rdaregistry.info/Elements/i/τρέχωνΙδιοκτήτης.el> ;
        skos:definition           "Συνδέει ένα αντίτυπο με έναν φορέα ο οποίος επί του παρόντος έχει τη νόμιμη κατοχή ενός αντιτύπου."@el ;
        rdakit:toolkitLabel       "τρέχων ιδιοκτήτης"@el ;
        rdakit:toolkitDefinition  "Ένας φορέας, ο οποίος επί του παρόντος έχει τη νόμιμη κατοχή ενός αντιτύπου."@el ;
        rdfs:label                "té com a propietari actual"@ca ;
        skos:definition           "Relaciona un item amb un agent que actualment posseeix legalment un ítem."@ca ;
        rdakit:toolkitLabel       "propietari actual"@ca ;
        rdakit:toolkitDefinition  "Agent que actualment posseeix legalment un ítem."@ca ;
        reg:name                  "nykyinenOmistaja"@fi ;
        rdfs:label                "nykyinen omistaja"@fi ;
        reg:lexicalAlias          <rdaa:nykyinenOmistaja.fi> ;
        skos:definition           "Liittää kappaleen toimijaan, joka nykyhetkellä laillisesti omistaa kappaleen."@fi ;
        rdakit:toolkitLabel       "nykyinen omistaja"@fi ;
        rdakit:toolkitDefinition  "Toimija, joka nykyhetkellä laillisesti omistaa kappaleen."@fi ;
        reg:name                  "propriétaireActuel"@fr ;
        reg:lexicalAlias          <http://rdaregistry.info/Elements/i/agentPropriétaireActuel.fr> ;
        rdakit:toolkitLabel       "nåværende eier"@no ;
        rdakit:toolkitDefinition  "En agent som for tiden er et eksemplars rettmessige eier."@no ;
        rdakit:hasElementType     "2" ;
        reg:name                  "jelenlegiTulajdonos"@hu ;
        rdfs:label                "van jelenlegi tulajdonosa"@hu ;
        skos:definition           "Egy példányt hozzákapcsol egy ágenshez (személyhez, családhoz vagy testülethez), akinek/amelynek  jogszerű tulajdonában van egy példány.  "@hu ;
        rdakit:toolkitLabel       "jelenlegi tulajdonos"@hu ;
        rdakit:toolkitDefinition  "Egy ágens (személy, család vagy testület), akinek/amelynek jelenleg jogos tulajdonában van egy példány."@hu ;
        skos:altLabel             "current owner"@en ;
        reg:hasSubproperty        <http://rdaregistry.info/Elements/i/P40107> ;
        reg:hasSubproperty        <http://rdaregistry.info/Elements/i/P40123> ;
        skos:altLabel             "propriétaire actuel"@fr .

<http://rdaregistry.info/Elements/i/P40117>
        rdfs:isDefinedBy          <http://rdaregistry.info/Elements/i/> ;
        reg:status                <http://metadataregistry.org/uri/RegStatus/1001> ;
        rdfs:label                "has current owner collective agent"@en ;
        reg:lexicalAlias          <http://rdaregistry.info/Elements/i/currentOwnerCollectiveAgent.en> ;
        skos:definition           "Relates an item to a collective agent who has current legal possession of an item."@en ;
        rdakit:toolkitLabel       "current owner collective agent"@en ;
        rdakit:toolkitDefinition  "A collective agent who has current legal possession of an item."@en ;
        rdf:type                  rdf:Property ;
        reg:name                  "currentOwnerCollectiveAgent" ;
        rdfs:domain               <http://rdaregistry.info/Elements/c/C10003> ;
        rdakit:hasElementType     "2" ;
        reg:hasSubproperty        <http://rdaregistry.info/Elements/i/datatype/P40117> ;
        reg:hasSubproperty        <http://rdaregistry.info/Elements/i/object/P40117> ;
        rdfs:subPropertyOf        <http://rdaregistry.info/Elements/i/P40120> ;
        rdfs:subPropertyOf        <http://rdaregistry.info/Elements/i/P40018> ;
        reg:hasSubproperty        <http://rdaregistry.info/Elements/i/P40123> ;
        reg:hasSubproperty        <http://rdaregistry.info/Elements/i/P40133> ;
        reg:hasSubproperty        <http://rdaregistry.info/Elements/i/P40149> ;
        reg:hasUnconstrained      <http://rdaregistry.info/Elements/u/P60400> ;
        rdfs:label                "a pour agent collectif propriétaire actuel"@fr ;
        skos:definition           "Met un item en relation avec un agent collectif qui possède actuellement et légalement un item."@fr ;
        rdakit:toolkitLabel       "agent collectif propriétaire actuel"@fr ;
        rdakit:toolkitDefinition  "Agent collectif qui possède actuellement et légalement un item."@fr ;
        reg:lexicalAlias          <http://rdaregistry.info/Elements/i/agentCollectifPropriétaireActuel.fr> .

<http://rdaregistry.info/Elements/i/P40133>
        rdfs:isDefinedBy          <http://rdaregistry.info/Elements/i/> ;
        reg:status                <http://metadataregistry.org/uri/RegStatus/1001> ;
        rdfs:label                "has current owner corporate body"@en ;
        reg:lexicalAlias          <http://rdaregistry.info/Elements/i/currentOwnerCorporateBody.en> ;
        skos:definition           "Relates an item to a corporate body who has current legal possession of an item."@en ;
        rdakit:toolkitLabel       "current owner corporate body"@en ;
        rdakit:toolkitDefinition  "A corporate body who has current legal possession of an item."@en ;
        rdf:type                  rdf:Property ;
        reg:name                  "currentOwnerCorporateBody" ;
        rdfs:domain               <http://rdaregistry.info/Elements/c/C10003> ;
        rdakit:hasElementType     "2" ;
        reg:hasSubproperty        <http://rdaregistry.info/Elements/i/datatype/P40133> ;
        reg:hasSubproperty        <http://rdaregistry.info/Elements/i/object/P40133> ;
        rdfs:subPropertyOf        <http://rdaregistry.info/Elements/i/P40136> ;
        rdfs:subPropertyOf        <http://rdaregistry.info/Elements/i/P40117> ;
        reg:hasSubproperty        <http://rdaregistry.info/Elements/i/P40139> ;
        reg:hasUnconstrained      <http://rdaregistry.info/Elements/u/P60400> ;
        rdfs:label                "a pour collectivité propriétaire actuelle"@fr ;
        skos:definition           "Met un item en relation avec une collectivité qui possède actuellement et légalement un item."@fr ;
        rdakit:toolkitLabel       "collectivité propriétaire actuelle"@fr ;
        rdakit:toolkitDefinition  "Collectivité qui possède actuellement et légalement un item."@fr ;
        reg:lexicalAlias          <http://rdaregistry.info/Elements/i/collectivitéPropriétaireActuelle.fr> .

<http://rdaregistry.info/Elements/i/P40149>
        rdfs:isDefinedBy          <http://rdaregistry.info/Elements/i/> ;
        reg:status                <http://metadataregistry.org/uri/RegStatus/1001> ;
        rdfs:label                "has current owner family"@en ;
        reg:lexicalAlias          <http://rdaregistry.info/Elements/i/currentOwnerFamily.en> ;
        skos:definition           "Relates an item to a family who has current legal possession of an item."@en ;
        rdakit:toolkitLabel       "current owner family"@en ;
        rdakit:toolkitDefinition  "A family who has current legal possession of an item."@en ;
        rdf:type                  rdf:Property ;
        reg:name                  "currentOwnerFamily" ;
        rdfs:domain               <http://rdaregistry.info/Elements/c/C10003> ;
        rdakit:hasElementType     "2" ;
        reg:hasSubproperty        <http://rdaregistry.info/Elements/i/datatype/P40149> ;
        reg:hasSubproperty        <http://rdaregistry.info/Elements/i/object/P40149> ;
        rdfs:subPropertyOf        <http://rdaregistry.info/Elements/i/P40152> ;
        rdfs:subPropertyOf        <http://rdaregistry.info/Elements/i/P40117> ;
        reg:hasSubproperty        <http://rdaregistry.info/Elements/i/P40155> ;
        reg:hasUnconstrained      <http://rdaregistry.info/Elements/u/P60400> ;
        rdfs:label                "a pour famille propriétaire actuelle"@fr ;
        skos:definition           "Met un item en relation avec une famille qui possède actuellement et légalement un item."@fr ;
        rdakit:toolkitLabel       "famille propriétaire actuelle"@fr ;
        rdakit:toolkitDefinition  "Famille qui possède actuellement et légalement un item."@fr ;
        reg:lexicalAlias          <http://rdaregistry.info/Elements/i/famillePropriétaireActuelle.fr> .

<http://rdaregistry.info/Elements/i/P40101>
        rdfs:isDefinedBy          <http://rdaregistry.info/Elements/i/> ;
        reg:status                <http://metadataregistry.org/uri/RegStatus/1001> ;
        rdfs:label                "has current owner person"@en ;
        reg:lexicalAlias          <http://rdaregistry.info/Elements/i/currentOwnerPerson.en> ;
        skos:definition           "Relates an item to a person who has current legal possession of an item."@en ;
        rdakit:toolkitLabel       "current owner person"@en ;
        rdakit:toolkitDefinition  "A person who has current legal possession of an item."@en ;
        rdf:type                  rdf:Property ;
        reg:name                  "currentOwnerPerson" ;
        rdfs:domain               <http://rdaregistry.info/Elements/c/C10003> ;
        rdakit:hasElementType     "2" ;
        reg:hasSubproperty        <http://rdaregistry.info/Elements/i/datatype/P40101> ;
        reg:hasSubproperty        <http://rdaregistry.info/Elements/i/object/P40101> ;
        rdfs:subPropertyOf        <http://rdaregistry.info/Elements/i/P40104> ;
        rdfs:subPropertyOf        <http://rdaregistry.info/Elements/i/P40018> ;
        reg:hasSubproperty        <http://rdaregistry.info/Elements/i/P40107> ;
        reg:hasUnconstrained      <http://rdaregistry.info/Elements/u/P60400> ;
        rdfs:label                "a pour personne propriétaire actuelle"@fr ;
        skos:definition           "Met un item en relation avec une personne qui possède actuellement et légalement un item."@fr ;
        rdakit:toolkitLabel       "personne propriétaire actuelle"@fr ;
        rdakit:toolkitDefinition  "Personne qui possède actuellement et légalement un item."@fr ;
        reg:lexicalAlias          <http://rdaregistry.info/Elements/i/personnePropriétaireActuelle.fr> .

<http://rdaregistry.info/Elements/i/P40026>
        rdfs:isDefinedBy          <http://rdaregistry.info/Elements/i/> ;
        reg:status                <http://metadataregistry.org/uri/RegStatus/1001> ;
        reg:name                  "custodialHistoryOfItem"@en ;
        rdfs:label                "has custodial history of item"@en ;
        skos:definition           "Relates an item to a record of previous ownership or custodianship of an item, including agent, place, and timespan."@en ;
        rdf:type                  rdf:Property ;
        rdfs:domain               <http://rdaregistry.info/Elements/c/C10003> ;
        reg:lexicalAlias          <http://rdaregistry.info/Elements/i/custodialHistoryOfItem.en> ;
        reg:hasUnconstrained      <http://rdaregistry.info/Elements/u/P60176> ;
        rdakit:instructionNumber  "2.18" ;
        rdakit:toolkitLabel       "custodial history of item"@en ;
        rdakit:toolkitDefinition  "A record of previous ownership or custodianship of an item, including agent, place, and timespan."@en ;
        rdfs:label                "a pour historique de la garde d’un item"@fr ;
        skos:definition           "Met un item en relation avec un enregistrement de la propriété ou de la garde antérieure d’un item, notamment un agent, un lieu et un laps de temps."@fr ;
        rdakit:toolkitLabel       "historique de la garde d’un item"@fr ;
        rdakit:toolkitDefinition  "Enregistrement de la propriété ou de la garde antérieure d’un item, notamment un agent, un lieu et un laps de temps."@fr ;
        rdakit:toolkitLabel       "historia de la custodia del ítem"@es ;
        rdakit:toolkitDefinition  "Un registro de la propiedad anterior o custodia de un ítem."@es ;
        reg:hasSubproperty        <http://rdaregistry.info/Elements/i/object/P40026> ;
        reg:name                  "lịchSửGiámHộCủaBản"@vi ;
        rdfs:label                "có lịch sử giám hộ của bản"@vi ;
        skos:definition           "Liên kết bản với với hồ sơ về quyền sở hữu hoặc quyền giám hộ trước đây của bản."@vi ;
        rdakit:toolkitLabel       "lịch sử giám hộ của bản"@vi ;
        rdakit:toolkitDefinition  "Với hồ sơ về quyền sở hữu hoặc quyền giám hộ trước đây của bản."@vi ;
        reg:name                  "proveniens"@da ;
        rdfs:label                "har proveniens af eksemplar"@da ;
        reg:lexicalAlias          <http://rdaregistry.info/Elements/i/proveniens.da> ;
        skos:definition           "Relaterer et eksemplar til en optegnelse over tidligere ejerskab eller opbevaring af et eksemplar."@da ;
        rdakit:toolkitLabel       "proveniens"@da ;
        rdakit:toolkitDefinition  "Optegnelse over tidligere ejerskab eller opbevaring af et eksemplar."@da ;
        rdfs:label                "hat Besitzhistorie des Exemplars"@de ;
        skos:definition           "Setzt ein Exemplar mit einem Bericht über frühere Eigentümer oder Verwahrer eines Exemplars in Beziehung."@de ;
        rdakit:toolkitLabel       "Besitzhistorie des Exemplars"@de ;
        rdakit:toolkitDefinition  "Ein Bericht über frühere Eigentümer oder Verwahrer eines Exemplars."@de ;
        reg:name                  "ιστορίαΘεματοφύλακαΤουΑντιτύπου"@el ;
        rdfs:label                "έχει ιστορία θεματοφύλακα του αντιτύπου"@el ;
        reg:lexicalAlias          <http://rdaregistry.info/Elements/i/ιστορίαΘεματοφύλακαΤουΑντιτύπου.el> ;
        skos:definition           "Συνδέει ένα αντίτυπο με μια εγγραφή της προηγούμενης ιδιοκτησίας ή της θεματοφυλακής ενός αντιτύπου."@el ;
        rdakit:toolkitLabel       "ιστορία του θεματοφύλακα του αντιτύπου"@el ;
        rdakit:toolkitDefinition  "Μια εγγραφή της προηγούμενης ιδιοκτησίας ή της θεματοφυλακής ενός αντιτύπου."@el ;
        rdfs:label                "té com a història de custòdia d’un ítem"@ca ;
        skos:definition           "Relaciona un item amb un registre dels propietaris anteriors o de la custòdia prèvia d’un ítem."@ca ;
        rdakit:toolkitLabel       "història de custòdia d’un ítem"@ca ;
        rdakit:toolkitDefinition  "Registre dels propietaris anteriors o de la custòdia prèvia d’un ítem."@ca ;
        reg:name                  "kappaleenOmistushistoria"@fi ;
        rdfs:label                "kappaleen omistushistoria"@fi ;
        reg:lexicalAlias          <rdaa:kappaleenOmistushistoria.fi> ;
        skos:definition           "Liittää kappaleen tietoihin kappaleen aiemmista omistajista tai säilyttäjistä."@fi ;
        rdakit:toolkitLabel       "kappaleen omistushistoria"@fi ;
        rdakit:toolkitDefinition  "Tietoja kappaleen aiemmista omistajista tai säilyttäjistä."@fi ;
        reg:name                  "historiqueDeLaGardeDunItem"@fr ;
        reg:lexicalAlias          <http://rdaregistry.info/Elements/i/historiqueDeLaGardeDunItem.fr> ;
        rdakit:toolkitLabel       "eksemplarets oppbevaringshistorikk"@no ;
        rdakit:toolkitDefinition  "En angivelse av tidligere eierforhold eller oppbevaring av et eksemplar."@no ;
        rdakit:hasElementType     "6" ;
        reg:name                  "Példányőrzéstörténete"@hu ;
        rdfs:label                "van példányőrzési története"@hu ;
        skos:definition           "Egy példányt hozzákapcsol egy példány korábbi tulajdonjogának vagy letétkezelésének nyilvántartásához."@hu ;
        rdakit:toolkitLabel       "példány őrzéstörténete"@hu ;
        rdakit:toolkitDefinition  "Egy példány korábbi tulajdonjogának vagy gondnokságának egy dokumentuma."@hu ;
        reg:hasSubproperty        <http://rdaregistry.info/Elements/i/datatype/P40026> .

<http://rdaregistry.info/Elements/i/P40020>
        rdfs:isDefinedBy          <http://rdaregistry.info/Elements/i/> ;
        reg:status                <http://metadataregistry.org/uri/RegStatus/1001> ;
        reg:name                  "custodianAgent"@en ;
        rdfs:label                "has custodian agent"@en ;
        skos:definition           "Relates an item to an agent who has legal custody of an item."@en ;
        rdf:type                  rdf:Property ;
        rdfs:domain               <http://rdaregistry.info/Elements/c/C10003> ;
        reg:lexicalAlias          <http://rdaregistry.info/Elements/i/custodianAgent.en> ;
        reg:hasUnconstrained      <http://rdaregistry.info/Elements/u/P60402> ;
        rdakit:instructionNumber  "22.3" ;
        rdakit:toolkitLabel       "custodian agent"@en ;
        rdakit:toolkitDefinition  "An agent who has legal custody of an item."@en ;
        rdfs:label                "a pour agent dépositaire"@fr ;
        skos:definition           "Met un item en relation avec un agent à qui est confiée la garde légale d’un item."@fr ;
        rdakit:toolkitLabel       "agent dépositaire"@fr ;
        rdakit:toolkitDefinition  "Agent à qui est confiée la garde légale d’un item."@fr ;
        rdakit:toolkitLabel       "custodio"@es ;
        rdakit:toolkitDefinition  "Una persona, familia o entidad corporativa que tiene la custodia legal de un ítem."@es ;
        rdfs:label                "har förvaltare"@sv ;
        rdakit:toolkitLabel       "förvaltare"@sv ;
        reg:hasSubproperty        <http://rdaregistry.info/Elements/i/object/P40020> ;
        rdfs:subPropertyOf        <http://rdaregistry.info/Elements/i/P40072> ;
        reg:name                  "ngườiGiámHộ"@vi ;
        rdfs:label                "có người giám hộ"@vi ;
        skos:definition           "Liên kết bản với tác nhân giám hộ theo pháp luật một bản."@vi ;
        rdakit:toolkitLabel       "người giám hộ"@vi ;
        rdakit:toolkitDefinition  "Tác nhân giám hộ theo pháp luật một bản."@vi ;
        reg:name                  "forvalter"@da ;
        rdfs:label                "har forvalter"@da ;
        reg:lexicalAlias          <http://rdaregistry.info/Elements/i/forvalter.da> ;
        skos:definition           "Relaterer et eksemplar til en agent, der lovligt har et eksemplar i forvaring."@da ;
        rdakit:toolkitLabel       "forvalter"@da ;
        rdakit:toolkitDefinition  "Agent, der lovligt har et eksemplar i forvaring."@da ;
        rdfs:label                "hat Verwahrer"@de ;
        skos:definition           "Setzt ein Exemplar mit einem Akteur, dem die rechtmäßige Verwahrung eines Exemplars obliegt, in Beziehung."@de ;
        rdakit:toolkitLabel       "Verwahrer"@de ;
        rdakit:toolkitDefinition  "Ein Akteur, dem die rechtmäßige Verwahrung eines Exemplars obliegt."@de ;
        reg:name                  "θεματοφύλακας"@el ;
        rdfs:label                "έχει θεματοφύλακα"@el ;
        reg:lexicalAlias          <http://rdaregistry.info/Elements/i/θεματοφύλακας.el> ;
        skos:definition           "Συνδέει ένα αντίτυπο με έναν φορέα που έχει τη νόμιμη επιμέλεια φύλαξης ενός αντιτύπου."@el ;
        rdakit:toolkitLabel       "θεματοφύλακας"@el ;
        rdakit:toolkitDefinition  "Ένας φορέας ο οποίος έχει τη νόμιμη επιμέλεια φύλαξης ενός αντιτύπου."@el ;
        rdfs:label                "té com a dipositari"@ca ;
        skos:definition           "Relaciona un item amb un agent que té la custodia legal d’un ítem."@ca ;
        rdakit:toolkitLabel       "dipositari"@ca ;
        rdakit:toolkitDefinition  "Agent que té la custodia legal d’un ítem."@ca ;
        reg:name                  "sailyttaja"@fi ;
        rdfs:label                "säilyttäjä"@fi ;
        reg:lexicalAlias          <rdaa:sailyttaja.fi> ;
        skos:definition           "Liittää kappaleen toimijaan, jolla on kappaleen laillinen säilyttämisoikeus."@fi ;
        rdakit:toolkitLabel       "säilyttäjä"@fi ;
        rdakit:toolkitDefinition  "Toimija, jolla on kappaleen laillinen säilyttämisoikeus."@fi ;
        reg:name                  "dépositaire"@fr ;
        reg:lexicalAlias          <http://rdaregistry.info/Elements/i/agentDépositaire.fr> ;
        rdakit:toolkitLabel       "oppbevarer"@no ;
        rdakit:toolkitDefinition  "En agent som har et eksemplar i lovlig forvaring."@no ;
        rdakit:hasElementType     "2" ;
        reg:name                  "gyűjteményvezető"@hu ;
        rdfs:label                "van gyűjteményvezetője"@hu ;
        skos:definition           "Egy példányt hozzákapcsol egy ágenshez (személyhez, családhoz vagy testülethez), akinek/amelynek jogi őrzésében van egy példány."@hu ;
        rdakit:toolkitLabel       "gyűjteményvezető"@hu ;
        rdakit:toolkitDefinition  "Egy ágens (személy, család vagy testület), akinek/amelynek jogos őrzésében van egy példány."@hu ;
        skos:altLabel             "custodian"@en ;
        skos:altLabel             "dépositaire"@fr .

<http://rdaregistry.info/Elements/i/P40119>
        rdfs:isDefinedBy          <http://rdaregistry.info/Elements/i/> ;
        reg:status                <http://metadataregistry.org/uri/RegStatus/1001> ;
        rdfs:label                "has custodian collective agent"@en ;
        reg:lexicalAlias          <http://rdaregistry.info/Elements/i/custodianCollectiveAgent.en> ;
        skos:definition           "Relates an item to a collective agent who has legal custody of an item."@en ;
        rdakit:toolkitLabel       "custodian collective agent"@en ;
        rdakit:toolkitDefinition  "A collective agent who has legal custody of an item."@en ;
        rdf:type                  rdf:Property ;
        reg:name                  "custodianCollectiveAgent" ;
        rdfs:domain               <http://rdaregistry.info/Elements/c/C10003> ;
        rdakit:hasElementType     "2" ;
        reg:hasSubproperty        <http://rdaregistry.info/Elements/i/datatype/P40119> ;
        reg:hasSubproperty        <http://rdaregistry.info/Elements/i/object/P40119> ;
        rdfs:subPropertyOf        <http://rdaregistry.info/Elements/i/P40076> ;
        rdfs:subPropertyOf        <http://rdaregistry.info/Elements/i/P40020> ;
        reg:hasSubproperty        <http://rdaregistry.info/Elements/i/P40135> ;
        reg:hasSubproperty        <http://rdaregistry.info/Elements/i/P40151> ;
        reg:hasUnconstrained      <http://rdaregistry.info/Elements/u/P60402> ;
        rdfs:label                "a pour agent collectif dépositaire"@fr ;
        skos:definition           "Met un item en relation avec un agent collectif à qui est confiée la garde légale d’un item."@fr ;
        rdakit:toolkitLabel       "agent collectif dépositaire"@fr ;
        rdakit:toolkitDefinition  "Agent collectif à qui est confiée la garde légale d’un item."@fr ;
        reg:lexicalAlias          <http://rdaregistry.info/Elements/i/agentCollectifDépositaire.fr> .

<http://rdaregistry.info/Elements/i/P40135>
        rdfs:isDefinedBy          <http://rdaregistry.info/Elements/i/> ;
        reg:status                <http://metadataregistry.org/uri/RegStatus/1001> ;
        rdfs:label                "has custodian corporate body"@en ;
        reg:lexicalAlias          <http://rdaregistry.info/Elements/i/custodianCorporateBody.en> ;
        skos:definition           "Relates an item to a corporate body who has legal custody of an item."@en ;
        rdakit:toolkitLabel       "custodian corporate body"@en ;
        rdakit:toolkitDefinition  "A corporate body who has legal custody of an item."@en ;
        rdf:type                  rdf:Property ;
        reg:name                  "custodianCorporateBody" ;
        rdfs:domain               <http://rdaregistry.info/Elements/c/C10003> ;
        rdakit:hasElementType     "2" ;
        reg:hasSubproperty        <http://rdaregistry.info/Elements/i/datatype/P40135> ;
        reg:hasSubproperty        <http://rdaregistry.info/Elements/i/object/P40135> ;
        rdfs:subPropertyOf        <http://rdaregistry.info/Elements/i/P40075> ;
        rdfs:subPropertyOf        <http://rdaregistry.info/Elements/i/P40119> ;
        reg:hasUnconstrained      <http://rdaregistry.info/Elements/u/P60402> ;
        rdfs:label                "a pour collectivité dédicataire"@fr ;
        skos:definition           "Met un item en relation avec une collectivité à qui est confiée la garde légale d’un item."@fr ;
        rdakit:toolkitLabel       "collectivité dédicataire"@fr ;
        rdakit:toolkitDefinition  "Collectivité à qui est confiée la garde légale d’un item."@fr ;
        reg:lexicalAlias          <http://rdaregistry.info/Elements/i/collectivitéDédicataire.fr> .

<http://rdaregistry.info/Elements/i/P40151>
        rdfs:isDefinedBy          <http://rdaregistry.info/Elements/i/> ;
        reg:status                <http://metadataregistry.org/uri/RegStatus/1001> ;
        rdfs:label                "has custodian family"@en ;
        reg:lexicalAlias          <http://rdaregistry.info/Elements/i/custodianFamily.en> ;
        skos:definition           "Relates an item to a family who has legal custody of an item."@en ;
        rdakit:toolkitLabel       "custodian family"@en ;
        rdakit:toolkitDefinition  "A family who has legal custody of an item."@en ;
        rdf:type                  rdf:Property ;
        reg:name                  "custodianFamily" ;
        rdfs:domain               <http://rdaregistry.info/Elements/c/C10003> ;
        rdakit:hasElementType     "2" ;
        reg:hasSubproperty        <http://rdaregistry.info/Elements/i/datatype/P40151> ;
        reg:hasSubproperty        <http://rdaregistry.info/Elements/i/object/P40151> ;
        rdfs:subPropertyOf        <http://rdaregistry.info/Elements/i/P40074> ;
        rdfs:subPropertyOf        <http://rdaregistry.info/Elements/i/P40119> ;
        reg:hasUnconstrained      <http://rdaregistry.info/Elements/u/P60402> ;
        rdfs:label                "a pour famille dédicataire"@fr ;
        skos:definition           "Met un item en relation avec une famille à qui est confiée la garde légale d’un item."@fr ;
        rdakit:toolkitLabel       "famille dédicataire"@fr ;
        rdakit:toolkitDefinition  "Famille à qui est confiée la garde légale d’un item."@fr ;
        reg:lexicalAlias          <http://rdaregistry.info/Elements/i/familleDédicataire.fr> .

<http://rdaregistry.info/Elements/i/P40103>
        rdfs:isDefinedBy          <http://rdaregistry.info/Elements/i/> ;
        reg:status                <http://metadataregistry.org/uri/RegStatus/1001> ;
        rdfs:label                "has custodian person"@en ;
        reg:lexicalAlias          <http://rdaregistry.info/Elements/i/custodianPerson.en> ;
        skos:definition           "Relates an item to a person who has legal custody of an item."@en ;
        rdakit:toolkitLabel       "custodian person"@en ;
        rdakit:toolkitDefinition  "A person who has legal custody of an item."@en ;
        rdf:type                  rdf:Property ;
        reg:name                  "custodianPerson" ;
        rdfs:domain               <http://rdaregistry.info/Elements/c/C10003> ;
        rdakit:hasElementType     "2" ;
        reg:hasSubproperty        <http://rdaregistry.info/Elements/i/datatype/P40103> ;
        reg:hasSubproperty        <http://rdaregistry.info/Elements/i/object/P40103> ;
        rdfs:subPropertyOf        <http://rdaregistry.info/Elements/i/P40073> ;
        rdfs:subPropertyOf        <http://rdaregistry.info/Elements/i/P40020> ;
        reg:hasUnconstrained      <http://rdaregistry.info/Elements/u/P60402> ;
        rdfs:label                "a pour personne dépositaire"@fr ;
        skos:definition           "Met un item en relation avec une personne à qui est confiée la garde légale d’un item."@fr ;
        rdakit:toolkitLabel       "personne dépositaire"@fr ;
        rdakit:toolkitDefinition  "Personne à qui est confiée la garde légale d’un item."@fr ;
        reg:lexicalAlias          <http://rdaregistry.info/Elements/i/personneDépositaire.fr> .

<http://rdaregistry.info/Elements/i/P40025>
        rdfs:isDefinedBy          <http://rdaregistry.info/Elements/i/> ;
        reg:status                <http://metadataregistry.org/uri/RegStatus/1001> ;
        reg:name                  "dedicateeAgentOfItem"@en ;
        rdfs:label                "has dedicatee agent of item"@en ;
        skos:definition           "Relates an item to an agent to whom an item is dedicated."@en ;
        rdf:type                  rdf:Property ;
        rdfs:domain               <http://rdaregistry.info/Elements/c/C10003> ;
        rdfs:subPropertyOf        <http://rdaregistry.info/Elements/i/P40072> ;
        reg:lexicalAlias          <http://rdaregistry.info/Elements/i/dedicateeAgentOfItem.en> ;
        reg:hasUnconstrained      <http://rdaregistry.info/Elements/u/P60455> ;
        rdakit:toolkitLabel       "dedicatee agent of item"@en ;
        rdakit:toolkitDefinition  "An agent to whom an item is dedicated."@en ;
        rdfs:label                "a pour agent dédicataire d’un item"@fr ;
        skos:definition           "Met un item en relation avec un agent à qui un item est dédié."@fr ;
        rdakit:toolkitLabel       "agent dédicataire d’un item"@fr ;
        rdakit:toolkitDefinition  "Agent à qui un item est dédié."@fr ;
        rdakit:toolkitLabel       "destinatario de dedicatoria en el ítem"@es ;
        rdakit:toolkitDefinition  "Una persona, familia o entidad corporativa a la cual se dedica un ítem."@es ;
        rdakit:instructionNumber  "18.5" ;
        reg:hasSubproperty        <http://rdaregistry.info/Elements/i/object/P40025> ;
        reg:name                  "ngườiĐượcĐềTặngCủaBản"@vi ;
        rdfs:label                "có người được đề tặng (bản)"@vi ;
        skos:definition           "Liên kết bản với tác nhân mà bản đề tặng."@vi ;
        rdakit:toolkitLabel       "người được đề tặng (bản)"@vi ;
        rdakit:toolkitDefinition  "Tác nhân mà bản đề tặng."@vi ;
        reg:name                  "tilegnetAfEksemplar"@da ;
        rdfs:label                "har tilegenet (eksemplar)"@da ;
        reg:lexicalAlias          <http://rdaregistry.info/Elements/i/tilegnetAfEksemplar.da> ;
        skos:definition           "Relaterer et eksemplar til en agent, som et eksemplar er tilegnet."@da ;
        rdakit:toolkitLabel       "tilegnet (eksemplar)"@da ;
        rdakit:toolkitDefinition  "Agent, som et eksemplar er tilegnet."@da ;
        rdfs:label                "hat Widmungsempfänger (Exemplar)"@de ;
        skos:definition           "Setzt ein Exemplar mit einem Akteur, dem ein Exemplar gewidmet ist, in Beziehung."@de ;
        rdakit:toolkitLabel       "Widmungsempfänger (Exemplar)"@de ;
        rdakit:toolkitDefinition  "Eine Akteur, dem ein Exemplar gewidmet ist."@de ;
        reg:name                  "αποδέκτηςΑφιέρωσηςΤουΑντιτύπου"@el ;
        rdfs:label                "έχει αποδέκτη αφιέρωσης (αντίτυπο)"@el ;
        reg:lexicalAlias          <http://rdaregistry.info/Elements/i/αποδέκτηςΑφιέρωσηςΤουΑντιτύπου.el> ;
        skos:definition           "Συνδέει ένα αντίτυπο με έναν φορέα στον οποίο είναι αφιερωμένο ένα αντίτυπο."@el ;
        rdakit:toolkitLabel       "αποδέκτης αφιέρωσης (αντίτυπο)"@el ;
        rdakit:toolkitDefinition  "Ένας φορέας στον οποίο είναι αφιερωμένο ένα αντίτυπο."@el ;
        rdfs:label                "té com a dedicatari (ítem)"@ca ;
        skos:definition           "Relaciona un item amb un agent a qui es dedica un ítem."@ca ;
        rdakit:toolkitLabel       "dedicatari (ítem)"@ca ;
        rdakit:toolkitDefinition  "Agent a qui es dedica un ítem."@ca ;
        reg:name                  "kappaleOmistettu"@fi ;
        rdfs:label                "kappale omistettu"@fi ;
        reg:lexicalAlias          <rdaa:kappaleOmistettu.fi> ;
        skos:definition           "Liittää kappaleen toimijaan, jolle kappale on omistettu."@fi ;
        rdakit:toolkitLabel       "kappale omistettu"@fi ;
        rdakit:toolkitDefinition  "Toimija, jolle kappale on omistettu."@fi ;
        reg:name                  "dédicataireItem"@fr ;
        reg:lexicalAlias          <http://rdaregistry.info/Elements/i/agentDédicataireDunItem.fr> ;
        rdakit:toolkitLabel       "tilegnet til (eksemplar)"@no ;
        rdakit:toolkitDefinition  "En agent som et eksemplar er dedisert til."@no ;
        rdakit:hasElementType     "2" ;
        reg:name                  "Példánydedikáltja"@hu ;
        rdfs:label                "van dedikáltja (példány)"@hu ;
        skos:definition           "Egy példányt hozzákapcsol egy ágenshez (személyhez, családhoz vagy testülethez), akinek/amelynek egy példányt ajánlanak."@hu ;
        rdakit:toolkitLabel       "ajánlás címzettje (pédány)"@hu ;
        rdakit:toolkitDefinition  "Egy ágens (személy, család vagy testület), akinek/amelynek egy példányt dedikáltak."@hu ;
        reg:hasSubproperty        <http://rdaregistry.info/Elements/i/datatype/P40025> ;
        skos:altLabel             "dedicatee (item)"@en ;
        skos:altLabel             "dédicataire (item)"@fr .

<http://rdaregistry.info/Elements/i/P40113>
        rdfs:isDefinedBy          <http://rdaregistry.info/Elements/i/> ;
        reg:status                <http://metadataregistry.org/uri/RegStatus/1001> ;
        rdfs:label                "has dedicatee collective agent of item"@en ;
        reg:lexicalAlias          <http://rdaregistry.info/Elements/i/dedicateeCollectiveAgentOfItem.en> ;
        skos:definition           "Relates an item to a collective agent to whom an item is dedicated."@en ;
        rdakit:toolkitLabel       "dedicatee collective agent of item"@en ;
        rdakit:toolkitDefinition  "A collective agent to whom an item is dedicated."@en ;
        rdf:type                  rdf:Property ;
        reg:name                  "dedicateeCollectiveAgentOfItem" ;
        rdfs:domain               <http://rdaregistry.info/Elements/c/C10003> ;
        rdakit:hasElementType     "2" ;
        reg:hasSubproperty        <http://rdaregistry.info/Elements/i/datatype/P40113> ;
        reg:hasSubproperty        <http://rdaregistry.info/Elements/i/object/P40113> ;
        rdfs:subPropertyOf        <http://rdaregistry.info/Elements/i/P40076> ;
        rdfs:subPropertyOf        <http://rdaregistry.info/Elements/i/P40025> ;
        reg:hasSubproperty        <http://rdaregistry.info/Elements/i/P40129> ;
        reg:hasSubproperty        <http://rdaregistry.info/Elements/i/P40145> ;
        reg:hasUnconstrained      <http://rdaregistry.info/Elements/u/P60455> ;
        rdfs:label                "a pour agent collectif dédicataire d’un item"@fr ;
        skos:definition           "Met un item en relation avec un agent collectif à qui un item est dédié."@fr ;
        rdakit:toolkitLabel       "agent collectif dédicataire d’un item"@fr ;
        rdakit:toolkitDefinition  "Agent collectif à qui un item est dédié."@fr ;
        reg:lexicalAlias          <http://rdaregistry.info/Elements/i/agentCollectifDédicataireDunItem.fr> .

<http://rdaregistry.info/Elements/i/P40129>
        rdfs:isDefinedBy          <http://rdaregistry.info/Elements/i/> ;
        reg:status                <http://metadataregistry.org/uri/RegStatus/1001> ;
        rdfs:label                "has dedicatee corporate body of item"@en ;
        reg:lexicalAlias          <http://rdaregistry.info/Elements/i/dedicateeCorporateBodyOfItem.en> ;
        skos:definition           "Relates an item to a corporate body to whom an item is dedicated."@en ;
        rdakit:toolkitLabel       "dedicatee corporate body of item"@en ;
        rdakit:toolkitDefinition  "A corporate body to whom an item is dedicated."@en ;
        rdf:type                  rdf:Property ;
        reg:name                  "dedicateeCorporateBodyOfItem" ;
        rdfs:domain               <http://rdaregistry.info/Elements/c/C10003> ;
        rdakit:hasElementType     "2" ;
        reg:hasSubproperty        <http://rdaregistry.info/Elements/i/datatype/P40129> ;
        reg:hasSubproperty        <http://rdaregistry.info/Elements/i/object/P40129> ;
        rdfs:subPropertyOf        <http://rdaregistry.info/Elements/i/P40075> ;
        rdfs:subPropertyOf        <http://rdaregistry.info/Elements/i/P40113> ;
        reg:hasUnconstrained      <http://rdaregistry.info/Elements/u/P60455> ;
        rdfs:label                "a pour collectivité dédicataire d’un item"@fr ;
        skos:definition           "Met un item en relation avec une collectivité à qui un item est dédié."@fr ;
        rdakit:toolkitLabel       "collectivité dédicataire d’un item"@fr ;
        rdakit:toolkitDefinition  "Collectivité à qui un item est dédié."@fr ;
        reg:lexicalAlias          <http://rdaregistry.info/Elements/i/collectivitéDédicataireDunItem.fr> .

<http://rdaregistry.info/Elements/i/P40145>
        rdfs:isDefinedBy          <http://rdaregistry.info/Elements/i/> ;
        reg:status                <http://metadataregistry.org/uri/RegStatus/1001> ;
        rdfs:label                "has dedicatee family of item"@en ;
        reg:lexicalAlias          <http://rdaregistry.info/Elements/i/dedicateeFamilyOfItem.en> ;
        skos:definition           "Relates an item to a family to whom an item is dedicated."@en ;
        rdakit:toolkitLabel       "dedicatee family of item"@en ;
        rdakit:toolkitDefinition  "A family to whom an item is dedicated."@en ;
        rdf:type                  rdf:Property ;
        reg:name                  "dedicateeFamilyOfItem" ;
        rdfs:domain               <http://rdaregistry.info/Elements/c/C10003> ;
        rdakit:hasElementType     "2" ;
        reg:hasSubproperty        <http://rdaregistry.info/Elements/i/datatype/P40145> ;
        reg:hasSubproperty        <http://rdaregistry.info/Elements/i/object/P40145> ;
        rdfs:subPropertyOf        <http://rdaregistry.info/Elements/i/P40074> ;
        rdfs:subPropertyOf        <http://rdaregistry.info/Elements/i/P40113> ;
        reg:hasUnconstrained      <http://rdaregistry.info/Elements/u/P60455> ;
        rdfs:label                "a pour famille dédicataire d’un item"@fr ;
        skos:definition           "Met un item en relation avec une famille à qui un item est dédié."@fr ;
        rdakit:toolkitLabel       "famille dédicataire d’un item"@fr ;
        rdakit:toolkitDefinition  "Famille à qui un item est dédié."@fr ;
        reg:lexicalAlias          <http://rdaregistry.info/Elements/i/familleDédicataireDunItem.fr> .

<http://rdaregistry.info/Elements/i/P40097>
        rdfs:isDefinedBy          <http://rdaregistry.info/Elements/i/> ;
        reg:status                <http://metadataregistry.org/uri/RegStatus/1001> ;
        rdfs:label                "has dedicatee person of item"@en ;
        reg:lexicalAlias          <http://rdaregistry.info/Elements/i/dedicateePersonOfItem.en> ;
        skos:definition           "Relates an item to a person to whom an item is dedicated."@en ;
        rdakit:toolkitLabel       "dedicatee person of item"@en ;
        rdakit:toolkitDefinition  "A person to whom an item is dedicated."@en ;
        rdf:type                  rdf:Property ;
        reg:name                  "dedicateePersonOfItem" ;
        rdfs:domain               <http://rdaregistry.info/Elements/c/C10003> ;
        rdakit:hasElementType     "2" ;
        reg:hasSubproperty        <http://rdaregistry.info/Elements/i/datatype/P40097> ;
        reg:hasSubproperty        <http://rdaregistry.info/Elements/i/object/P40097> ;
        rdfs:subPropertyOf        <http://rdaregistry.info/Elements/i/P40073> ;
        rdfs:subPropertyOf        <http://rdaregistry.info/Elements/i/P40025> ;
        reg:hasUnconstrained      <http://rdaregistry.info/Elements/u/P60455> ;
        rdfs:label                "a pour personne dédicataire d’un item"@fr ;
        skos:definition           "Met un item en relation avec une personne à qui un item est dédié."@fr ;
        rdakit:toolkitLabel       "personne dédicataire d’un item"@fr ;
        rdakit:toolkitDefinition  "Personne à qui un item est dédié."@fr ;
        reg:lexicalAlias          <http://rdaregistry.info/Elements/i/personneDédicataireDunItem.fr> .

<http://rdaregistry.info/Elements/i/P40006>
        rdfs:isDefinedBy          <http://rdaregistry.info/Elements/i/> ;
        reg:status                <http://metadataregistry.org/uri/RegStatus/1001> ;
        reg:name                  "depositorAgent"@en ;
        rdfs:label                "has depositor agent"@en ;
        skos:definition           "Relates an item to an agent who is a current owner of an item who deposits the item into the custody of another agent without transferring ownership."@en ;
        rdf:type                  rdf:Property ;
        rdfs:domain               <http://rdaregistry.info/Elements/c/C10003> ;
        rdfs:subPropertyOf        <http://rdaregistry.info/Elements/i/P40018> ;
        reg:lexicalAlias          <http://rdaregistry.info/Elements/i/depositorAgent.en> ;
        reg:hasUnconstrained      <http://rdaregistry.info/Elements/u/P60068> ;
        rdakit:toolkitLabel       "depositor agent"@en ;
        rdakit:toolkitDefinition  "An agent who is a current owner of an item who deposits the item into the custody of another agent without transferring ownership."@en ;
        rdfs:label                "a pour agent déposant"@fr ;
        skos:definition           "Met un item en relation avec un agent propriétaire actuel d’un item qui dépose l’item sous la garde d’un autre agent sans en transférer la propriété."@fr ;
        rdakit:toolkitLabel       "agent déposant"@fr ;
        rdakit:toolkitDefinition  "Agent propriétaire actuel d’un item qui dépose l’item sous la garde d’un autre agent sans en transférer la propriété."@fr ;
        rdakit:toolkitLabel       "depositante"@es ;
        rdakit:toolkitDefinition  "Un propietario actual de un ítem que lo entrega en custodia a otra persona, familia o entidad corporativa, sin perder la propiedad del ítem."@es ;
        rdakit:instructionNumber  "18.5" ;
        reg:hasSubproperty        <http://rdaregistry.info/Elements/i/object/P40006> ;
        reg:name                  "ngườiGửiĐồVật"@vi ;
        rdfs:label                "có người gửi đồ vật"@vi ;
        skos:definition           "Liên kết bản với người chủ hiện tại của bản, người đã nộp bản đó cho sự chăm nom của tác nhân khác trong khi vẫn giữa quyền sở hữu."@vi ;
        rdakit:toolkitLabel       "người gửi đồ vật"@vi ;
        rdakit:toolkitDefinition  "Người chủ hiện tại của bản, người đã nộp bản đó cho sự chăm nom của tác nhân khác trong khi vẫn giữa quyền sở hữu."@vi ;
        reg:name                  "udlåner"@da ;
        rdfs:label                "har udlåner"@da ;
        reg:lexicalAlias          <http://rdaregistry.info/Elements/i/udlåner.da> ;
        skos:definition           "Relaterer et eksemplar til en nuværende ejer af et eksemplar, der har deponeret eksemplaret til forvaring hos en anden person, familie eller korporation, men som fortsat har ejendomsretten."@da ;
        rdakit:toolkitLabel       "udlåner"@da ;
        rdakit:toolkitDefinition  "Nuværende ejer af et eksemplar, der har deponeret eksemplaret til forvaring hos en anden person, familie eller korporation, men som fortsat har ejendomsretten."@da ;
        rdfs:label                "hat Leihgeber"@de ;
        skos:definition           "Setzt ein Exemplar mit einem gegenwärtigen Eigentümer eines Exemplars, der ein Exemplar in die Obhut eines anderen Akteurs gegeben hat, während er weiterhin der Eigentümer bleibt, in Beziehung."@de ;
        rdakit:toolkitLabel       "Leihgeber"@de ;
        rdakit:toolkitDefinition  "Gegenwärtiger Eigentümer eines Exemplars, der ein Exemplar in die Obhut eines anderen Akteurs gegeben hat, während er weiterhin der Eigentümer bleibt."@de ;
        reg:name                  "καταθέτης"@el ;
        rdfs:label                "έχει καταθέτη"@el ;
        reg:lexicalAlias          <http://rdaregistry.info/Elements/i/καταθέτης.el> ;
        skos:definition           "Συνδέει ένα αντίτυπο με έναν τρέχοντα ιδιοκτήτη ενός αντιτύπου ο οποίος κατέθεσε το αντίτυπο υπό τη διαχειριστική επιτροπεία κάποιου άλλου φορέα, ενώ διατηρεί ακόμη την ιδιοκτησία."@el ;
        rdakit:toolkitLabel       "καταθέτης"@el ;
        rdakit:toolkitDefinition  "Ένας τρέχων ιδιοκτήτης ενός αντιτύπου, ο οποίος κατέθεσε το αντίτυπο υπό τη διαχειριστική επιτροπεία κάποιου άλλου φορέα, ενώ διατηρεί ακόμη την ιδιοκτησία."@el ;
        rdfs:label                "té com a dipositari"@ca ;
        skos:definition           "Relaciona un item amb un propietari actual d’un ítem que el diposita sota la custòdia d’un altre agent, mentre en reté la propietat."@ca ;
        rdakit:toolkitLabel       "dipositari"@ca ;
        rdakit:toolkitDefinition  "Propietari actual d’un ítem que el diposita sota la custòdia d’un altre agent, mentre en reté la propietat."@ca ;
        reg:name                  "tallettaja"@fi ;
        rdfs:label                "tallettaja"@fi ;
        reg:lexicalAlias          <rdaa:tallettaja.fi> ;
        skos:definition           "Liittää kappaleen sen nykyiseen omistajaan, joka on antanut sen toisen toimijan hallintaan, vaikka laillisesti omistaa kappaleen."@fi ;
        rdakit:toolkitLabel       "tallettaja"@fi ;
        rdakit:toolkitDefinition  "Kappaleen nykyinen omistaja, joka on antanut sen toisen toimijan hallintaan, vaikka laillisesti omistaa kappaleen."@fi ;
        reg:name                  "déposant"@fr ;
        reg:lexicalAlias          <http://rdaregistry.info/Elements/i/agentDéposant.fr> ;
        rdakit:toolkitLabel       "deponent"@no ;
        rdakit:toolkitDefinition  "En nåværende eier av et eksemplar som har deponert eksemplaret hos en annen agent som har eksemplaret i forvaring mens deponenten forblir eier."@no ;
        rdakit:hasElementType     "2" ;
        reg:name                  "letétbehelyező"@hu ;
        rdfs:label                "van letétbehelyezője"@hu ;
        skos:definition           "Egy példányt hozzákapcsol egy példány jelenlegi tulajdonosához, aki egy másik ágens (személy, család vagy testület) őrzésére letétbe helyezte a példányt, miközben megtartotta annak tulajdonjogát."@hu ;
        rdakit:toolkitLabel       "letétbehelyező"@hu ;
        rdakit:toolkitDefinition  "Egy példány jelenlegi tulajdonosa, aki egy másik ágens (személy, család vagy testület) őrizetébe helyezte a példányt, ugyanakkor a tulajdonjogot megtartotta. "@hu ;
        skos:altLabel             "depositor"@en ;
        skos:altLabel             "déposant"@fr .

<http://rdaregistry.info/Elements/i/P40123>
        rdfs:isDefinedBy          <http://rdaregistry.info/Elements/i/> ;
        reg:status                <http://metadataregistry.org/uri/RegStatus/1001> ;
        rdfs:label                "has depositor collective agent"@en ;
        reg:lexicalAlias          <http://rdaregistry.info/Elements/i/depositorCollectiveAgent.en> ;
        skos:definition           "Relates an item to a collective agent who is a current owner of an item who deposits the item into the custody of another agent without transferring ownership."@en ;
        rdakit:toolkitLabel       "depositor collective agent"@en ;
        rdakit:toolkitDefinition  "A collective agent who is a current owner of an item who deposits the item into the custody of another agent without transferring ownership."@en ;
        rdf:type                  rdf:Property ;
        reg:name                  "depositorCollectiveAgent" ;
        rdfs:domain               <http://rdaregistry.info/Elements/c/C10003> ;
        rdakit:hasElementType     "2" ;
        reg:hasSubproperty        <http://rdaregistry.info/Elements/i/datatype/P40123> ;
        reg:hasSubproperty        <http://rdaregistry.info/Elements/i/object/P40123> ;
        rdfs:subPropertyOf        <http://rdaregistry.info/Elements/i/P40117> ;
        rdfs:subPropertyOf        <http://rdaregistry.info/Elements/i/P40006> ;
        reg:hasSubproperty        <http://rdaregistry.info/Elements/i/P40139> ;
        reg:hasSubproperty        <http://rdaregistry.info/Elements/i/P40155> ;
        reg:hasUnconstrained      <http://rdaregistry.info/Elements/u/P60068> ;
        rdfs:label                "a pour agent collectif déposant"@fr ;
        skos:definition           "Met un item en relation avec un agent collectif propriétaire actuel d’un item qui dépose l’item sous la garde d’un autre agent sans en transférer la propriété."@fr ;
        rdakit:toolkitLabel       "agent collectif déposant"@fr ;
        rdakit:toolkitDefinition  "Agent collectif propriétaire actuel d’un item qui dépose l’item sous la garde d’un autre agent sans en transférer la propriété."@fr ;
        reg:lexicalAlias          <http://rdaregistry.info/Elements/i/agentCollectifDéposant.fr> .

<http://rdaregistry.info/Elements/i/P40139>
        rdfs:isDefinedBy          <http://rdaregistry.info/Elements/i/> ;
        reg:status                <http://metadataregistry.org/uri/RegStatus/1001> ;
        rdfs:label                "has depositor corporate body"@en ;
        reg:lexicalAlias          <http://rdaregistry.info/Elements/i/depositorCorporateBody.en> ;
        skos:definition           "Relates an item to a corporate body who is a current owner of an item who deposits the item into the custody of another agent without transferring ownership."@en ;
        rdakit:toolkitLabel       "depositor corporate body"@en ;
        rdakit:toolkitDefinition  "A corporate body who is a current owner of an item who deposits the item into the custody of another agent without transferring ownership."@en ;
        rdf:type                  rdf:Property ;
        reg:name                  "depositorCorporateBody" ;
        rdfs:domain               <http://rdaregistry.info/Elements/c/C10003> ;
        rdakit:hasElementType     "2" ;
        reg:hasSubproperty        <http://rdaregistry.info/Elements/i/datatype/P40139> ;
        reg:hasSubproperty        <http://rdaregistry.info/Elements/i/object/P40139> ;
        rdfs:subPropertyOf        <http://rdaregistry.info/Elements/i/P40133> ;
        rdfs:subPropertyOf        <http://rdaregistry.info/Elements/i/P40123> ;
        reg:hasUnconstrained      <http://rdaregistry.info/Elements/u/P60068> ;
        rdfs:label                "a pour collectivité déposante"@fr ;
        skos:definition           "Met un item en relation avec une collectivité propriétaire actuelle d’un item qui dépose l’item sous la garde d’un autre agent sans en transférer la propriété."@fr ;
        rdakit:toolkitLabel       "collectivité déposante"@fr ;
        rdakit:toolkitDefinition  "Collectivité propriétaire actuelle d’un item qui dépose l’item sous la garde d’un autre agent sans en transférer la propriété."@fr ;
        reg:lexicalAlias          <http://rdaregistry.info/Elements/i/collectivitéDéposante.fr> .

<http://rdaregistry.info/Elements/i/P40155>
        rdfs:isDefinedBy          <http://rdaregistry.info/Elements/i/> ;
        reg:status                <http://metadataregistry.org/uri/RegStatus/1001> ;
        rdfs:label                "has depositor family"@en ;
        reg:lexicalAlias          <http://rdaregistry.info/Elements/i/depositorFamily.en> ;
        skos:definition           "Relates an item to a family who is a current owner of an item who deposits the item into the custody of another agent without transferring ownership."@en ;
        rdakit:toolkitLabel       "depositor family"@en ;
        rdakit:toolkitDefinition  "A family who is a current owner of an item who deposits the item into the custody of another agent without transferring ownership."@en ;
        rdf:type                  rdf:Property ;
        reg:name                  "depositorFamily" ;
        rdfs:domain               <http://rdaregistry.info/Elements/c/C10003> ;
        rdakit:hasElementType     "2" ;
        reg:hasSubproperty        <http://rdaregistry.info/Elements/i/datatype/P40155> ;
        reg:hasSubproperty        <http://rdaregistry.info/Elements/i/object/P40155> ;
        rdfs:subPropertyOf        <http://rdaregistry.info/Elements/i/P40149> ;
        rdfs:subPropertyOf        <http://rdaregistry.info/Elements/i/P40123> ;
        reg:hasUnconstrained      <http://rdaregistry.info/Elements/u/P60068> ;
        rdfs:label                "a pour famille déposante"@fr ;
        skos:definition           "Met un item en relation avec une famille propriétaire actuelle d’un item qui dépose l’item sous la garde d’un autre agent sans en transférer la propriété."@fr ;
        rdakit:toolkitLabel       "famille déposante"@fr ;
        rdakit:toolkitDefinition  "Famille propriétaire actuelle d’un item qui dépose l’item sous la garde d’un autre agent sans en transférer la propriété."@fr ;
        reg:lexicalAlias          <http://rdaregistry.info/Elements/i/familleDéposante.fr> .

<http://rdaregistry.info/Elements/i/P40107>
        rdfs:isDefinedBy          <http://rdaregistry.info/Elements/i/> ;
        reg:status                <http://metadataregistry.org/uri/RegStatus/1001> ;
        rdfs:label                "has depositor person"@en ;
        reg:lexicalAlias          <http://rdaregistry.info/Elements/i/depositorPerson.en> ;
        skos:definition           "Relates an item to a person who is a current owner of an item who deposits the item into the custody of another agent without transferring ownership."@en ;
        rdakit:toolkitLabel       "depositor person"@en ;
        rdakit:toolkitDefinition  "A person who is a current owner of an item who deposits the item into the custody of another agent without transferring ownership."@en ;
        rdf:type                  rdf:Property ;
        reg:name                  "depositorPerson" ;
        rdfs:domain               <http://rdaregistry.info/Elements/c/C10003> ;
        rdakit:hasElementType     "2" ;
        reg:hasSubproperty        <http://rdaregistry.info/Elements/i/datatype/P40107> ;
        reg:hasSubproperty        <http://rdaregistry.info/Elements/i/object/P40107> ;
        rdfs:subPropertyOf        <http://rdaregistry.info/Elements/i/P40101> ;
        rdfs:subPropertyOf        <http://rdaregistry.info/Elements/i/P40006> ;
        reg:hasUnconstrained      <http://rdaregistry.info/Elements/u/P60068> ;
        rdfs:label                "a pour personne déposante"@fr ;
        skos:definition           "Met un item en relation avec une personne propriétaire actuelle d’un item qui dépose l’item sous la garde d’un autre agent sans en transférer la propriété."@fr ;
        rdakit:toolkitLabel       "personne déposante"@fr ;
        rdakit:toolkitDefinition  "Personne propriétaire actuelle d’un item qui dépose l’item sous la garde d’un autre agent sans en transférer la propriété."@fr ;
        reg:lexicalAlias          <http://rdaregistry.info/Elements/i/personneDéposante.fr> .

<http://rdaregistry.info/Elements/i/P40030>
        rdfs:isDefinedBy    <http://rdaregistry.info/Elements/i/> ;
        reg:status          <http://metadataregistry.org/uri/RegStatus/1008> ;
        rdf:type            rdf:Property ;
        rdfs:subPropertyOf  <http://rdaregistry.info/Elements/i/P40052> ;
        reg:hasSubproperty  <http://rdaregistry.info/Elements/i/P40033> ;
        reg:hasSubproperty  <http://rdaregistry.info/Elements/i/P40037> ;
        reg:hasSubproperty  <http://rdaregistry.info/Elements/i/P40040> ;
        reg:hasSubproperty  <http://rdaregistry.info/Elements/i/P40041> ;
        reg:hasSubproperty  <http://rdaregistry.info/Elements/i/P40043> .

<http://rdaregistry.info/Elements/i/P40056>
        rdfs:isDefinedBy          <http://rdaregistry.info/Elements/i/> ;
        reg:status                <http://metadataregistry.org/uri/RegStatus/1008> ;
        rdf:type                  rdf:Property ;
        rdfs:domain               <http://rdaregistry.info/Elements/c/C10003> ;
        reg:hasUnconstrained      <http://rdaregistry.info/Elements/u/P60200> ;
        rdfs:label                "a pour transfert numérique (item)"@fr ;
        skos:definition           "Met un item en relation avec un item en format numérique qui résulte du transfert d’un item dans un format numérique différent."@fr ;
        rdakit:toolkitLabel       "transfert numérique (item)"@fr ;
        rdakit:toolkitDefinition  "Item en format numérique qui résulte du transfert d’un item dans un format numérique différent."@fr ;
        rdakit:toolkitLabel       "transferencia digital (ítem)"@es ;
        rdakit:toolkitDefinition  "Un ítem en un formato digital que resulta de la transferencia de un ítem en otro formato digital."@es ;
        rdfs:subPropertyOf        <http://rdaregistry.info/Elements/i/P40055> ;
        rdakit:instructionNumber  "24.5" ;
        reg:hasSubproperty        <http://rdaregistry.info/Elements/i/object/P40056> ;
        reg:name                  "bảnChuyểnKỹThuậtSố"@vi ;
        rdfs:label                "có chuyển kỹ thuật số (bản)"@vi ;
        skos:definition           "Liên kết bản với bản dưới định dạng số là kết quả của việc chuyển ạng của bản dưới định dạng số khác."@vi ;
        rdakit:toolkitLabel       "chuyển kỹ thuật số (bản)"@vi ;
        rdakit:toolkitDefinition  "Bản dưới định dạng số là kết quả của việc chuyển ạng của bản dưới định dạng số khác."@vi ;
        reg:name                  "digitalOverførselEksemplar"@da ;
        rdfs:label                "har digital overførsel (eksemplar)"@da ;
        reg:lexicalAlias          <http://rdaregistry.info/Elements/i/digitalOverførselEksemplar.da> ;
        skos:definition           "Relaterer et eksemplar til et eksemplar i et digitalt format, der er resultatet af overførsel af et eksemplar i et andet digitalt format."@da ;
        rdakit:toolkitLabel       "digital overførsel (eksemplar)"@da ;
        rdakit:toolkitDefinition  "Eksemplar i et digitalt format, der er resultatet af overførsel af et eksemplar i et andet digitalt format."@da ;
        rdfs:label                "hat digitale Übertragung (Exemplar)"@de ;
        skos:definition           "Setzt ein Exemplar mit einem Exemplar in einem digitalen Format, das aus der Übertragung eines Exemplars in ein anderes digitales Format resultiert, in Beziehung."@de ;
        rdakit:toolkitLabel       "Digitale Übertragung (Exemplar)"@de ;
        rdakit:toolkitDefinition  "Ein Exemplar in einem digitalen Format, das aus der Übertragung eines Exemplars in ein anderes digitales Format resultiert."@de ;
        reg:name                  "ψηφιακήΜεταφοράΑντιτύπου"@el ;
        rdfs:label                "έχει ψηφιακή μεταφορά (αντίτυπο)"@el ;
        reg:lexicalAlias          <http://rdaregistry.info/Elements/i/ψηφιακήΜεταφοράΑντιτύπου.el> ;
        skos:definition           "Συνδέει ένα αντίτυπο με ένα αντίτυπο σε ένα ψηφιακό μορφότυπο το οποίο προκύπτει από τη μεταφορά ενός αντιτύπου σε ένα άλλο ψηφιακό μορφότυπο."@el ;
        rdakit:toolkitLabel       "ψηφιακή μεταφορά (αντίτυπο)"@el ;
        rdakit:toolkitDefinition  "Ένα αντίτυπο σε ψηφιακό μορφότυπο το οποίο προκύπτει από τη μεταφορά ενός αντιτύπου σε ένα άλλο ψηφιακό μορφότυπο."@el ;
        rdfs:label                "té com a transferència digital (ítem)"@ca ;
        skos:definition           "Relaciona un item amb un ítem en un format digital que és el resultat de la transferència d’un ítem en un altre format digital."@ca ;
        rdakit:toolkitLabel       "transferència digital (ítem)"@ca ;
        rdakit:toolkitDefinition  "Ítem en un format digital que és el resultat de la transferència d’un ítem en un altre format digital."@ca ;
        reg:name                  "konvertoitunaKappale"@fi ;
        rdfs:label                "konvertoituna (kappale)"@fi ;
        reg:lexicalAlias          <rdaa:konvertoitunaKappale.fi> ;
        skos:definition           "Liittää kappaleen digitaalisessa muodossa olevaan kappaleeseen, joka syntyy toisen digitaalisessa muodossa olevan kappaleen digitoinnin tuloksena."@fi ;
        rdakit:toolkitLabel       "konvertoituna (kappale)"@fi ;
        rdakit:toolkitDefinition  "Digitaalisessa muodossa oleva kappale, joka syntyy toisen digitaalisessa muodossa olevan kappaleen digitoinnin tuloksena."@fi ;
        reg:name                  "transfertNumériqueItem"@fr ;
        reg:lexicalAlias          <http://rdaregistry.info/Elements/i/transfertNumériqueItem.fr> ;
        rdakit:toolkitLabel       "digital overføring (eksemplar)"@no ;
        rdakit:toolkitDefinition  "Et eksemplar i digitalt format som er resultatet av overføring av et eksemplar fra et annet digitalt format."@no ;
        reg:hasSubproperty        <http://rdaregistry.info/Elements/i/datatype/P40056> .

<http://rdaregistry.info/Elements/i/P40087>
        rdfs:isDefinedBy          <http://rdaregistry.info/Elements/i/> ;
        reg:status                <http://metadataregistry.org/uri/RegStatus/1001> ;
        rdfs:label                "has digital transfer of item"@en ;
        rdf:type                  rdf:Property ;
        reg:name                  "digitalTransferOfItem"@en ;
        reg:lexicalAlias          <http://rdaregistry.info/Elements/i/digitalTransferOfItem.en> ;
        skos:definition           "Relates an item to a manifestation in a digital format that results from the transfer of an item in another digital format."@en ;
        rdfs:domain               <http://rdaregistry.info/Elements/c/C10003> ;
        rdfs:subPropertyOf        <http://rdaregistry.info/Elements/i/P40092> ;
        rdakit:toolkitLabel       "digital transfer of item"@en ;
        rdakit:toolkitDefinition  "A manifestation in a digital format that results from the transfer of an item in another digital format."@en ;
        reg:hasUnconstrained      <http://rdaregistry.info/Elements/u/P60200> ;
        rdakit:hasElementType     "2" ;
        reg:hasSubproperty        <http://rdaregistry.info/Elements/i/datatype/P40087> ;
        rdfs:label                "a pour transfert numérique d’un item"@fr ;
        skos:definition           "Met un item en relation avec une manifestation en format numérique qui résulte du transfert d’un item dans un format numérique différent."@fr ;
        rdakit:toolkitLabel       "transfert numérique d’un item"@fr ;
        rdakit:toolkitDefinition  "Manifestation en format numérique qui résulte du transfert d’un item dans un format numérique différent."@fr ;
        reg:lexicalAlias          <http://rdaregistry.info/Elements/i/transfertNumériqueDunItem.fr> ;
        skos:altLabel             "digital transfer (item)"@en .

<http://rdaregistry.info/Elements/i/P40039>
        rdfs:isDefinedBy          <http://rdaregistry.info/Elements/i/> ;
        reg:status                <http://metadataregistry.org/uri/RegStatus/1008> ;
        rdf:type                  rdf:Property ;
        rdfs:domain               <http://rdaregistry.info/Elements/c/C10003> ;
        rdfs:subPropertyOf        <http://rdaregistry.info/Elements/i/P40042> ;
        reg:hasUnconstrained      <http://rdaregistry.info/Elements/u/P60287> ;
        rdfs:label                "est un transfert numérique de (item)"@fr ;
        skos:definition           "Met un item en relation avec un item en format numérique qui a été transféré dans un format numérique différent."@fr ;
        rdakit:toolkitLabel       "transfert numérique de (item)"@fr ;
        rdakit:toolkitDefinition  "Item en format numérique qui a été transféré dans un format numérique différent."@fr ;
        rdakit:toolkitLabel       "transferencia digital de (ítem)"@es ;
        rdakit:toolkitDefinition  "Un ítem en un formato digital que es transferido a otro formato digital."@es ;
        rdakit:instructionNumber  "24.5" ;
        reg:hasSubproperty        <http://rdaregistry.info/Elements/i/object/P40039> ;
        reg:name                  "bảnChuyềnĐiệnTửCủaBản"@vi ;
        rdfs:label                "là bản chuyền điện tử của (bản)"@vi ;
        skos:definition           "Liên kết bản với bản dưới định dạng số được chuyển sang định dạng số khác."@vi ;
        rdakit:toolkitLabel       "bản chuyền điện tử của (bản)"@vi ;
        rdakit:toolkitDefinition  "Bản dưới định dạng số được chuyển sang định dạng số khác."@vi ;
        reg:name                  "digitalOverførselAfEksemplar"@da ;
        rdfs:label                "er digital overførsel af (eksemplar)"@da ;
        reg:lexicalAlias          <http://rdaregistry.info/Elements/i/digitalOverførselAfEksemplar.da> ;
        skos:definition           "Relaterer et eksemplar til et eksemplar i et digitalt format, der er overført til et andet digitalt format."@da ;
        rdakit:toolkitLabel       "digital overførsel af (eksemplar)"@da ;
        rdakit:toolkitDefinition  "Eksemplar i et digitalt format, der er overført til et andet digitalt format."@da ;
        rdfs:label                "ist digitale Übertragung von (Exemplar)"@de ;
        skos:definition           "Setzt ein Exemplar mit einem Exemplar in einem digitalen Format, das in ein anderes digitales Format übertragen wurde, in Beziehung."@de ;
        rdakit:toolkitLabel       "Digitale Übertragung von (Exemplar)"@de ;
        rdakit:toolkitDefinition  "Ein Exemplar in einem digitalen Format, das in ein anderes digitales Format übertragen wurde."@de ;
        reg:name                  "ψηφιακήΜεταφοράΤουΑντιτύπου"@el ;
        rdfs:label                "είναι ψηφιακή μεταφορά του (αντίτυπο)"@el ;
        reg:lexicalAlias          <http://rdaregistry.info/Elements/i/ψηφιακήΜεταφοράΤουΑντιτύπου.el> ;
        skos:definition           "Συνδέει ένα αντίτυπο με ένα αντίτυπο σε ένα ψηφιακό μορφότυπο που μεταφέρεται σε ένα άλλο ψηφιακό μορφότυπο."@el ;
        rdakit:toolkitLabel       "ψηφιακή μεταφορά του (αντίτυπο)"@el ;
        rdakit:toolkitDefinition  "Ένα αντίτυπο σε ένα ψηφιακό μορφότυπο που μεταφέρεται σε ένα άλλο ψηφιακό μορφότυπο."@el ;
        rdfs:label                "és transferència digital de (ítem)"@ca ;
        skos:definition           "Relaciona un item amb un ítem en un format digital que es transfereix a un altre format digital."@ca ;
        rdakit:toolkitLabel       "transferència digital de (ítem)"@ca ;
        rdakit:toolkitDefinition  "Ítem en un format digital que es transfereix a un altre format digital."@ca ;
        reg:name                  "konvertoituKappaleesta"@fi ;
        rdfs:label                "konvertoitu kappaleesta"@fi ;
        reg:lexicalAlias          <rdaa:konvertoituKappaleesta.fi> ;
        skos:definition           "Liittää kappaleen digitaalisessa muodossa olevaan kappaleeseen, jota on muunnettu toiseen digitaaliseen muotoon."@fi ;
        rdakit:toolkitLabel       "konvertoitu kappaleesta"@fi ;
        rdakit:toolkitDefinition  "Digitaalisessa muodossa oleva kappale, jota on muunnettu toiseen digitaaliseen muotoon."@fi ;
        reg:name                  "transfertNumériqueDeItem"@fr ;
        reg:lexicalAlias          <http://rdaregistry.info/Elements/i/transfertNumériqueDeItem.fr> ;
        rdakit:toolkitLabel       "digital overføring av (eksemplar)"@no ;
        rdakit:toolkitDefinition  "Et eksemplar i et digitalt format som overføres til et annet digitalt format."@no ;
        reg:hasSubproperty        <http://rdaregistry.info/Elements/i/datatype/P40039> .

<http://rdaregistry.info/Elements/i/P40007>
        rdfs:isDefinedBy          <http://rdaregistry.info/Elements/i/> ;
        reg:status                <http://metadataregistry.org/uri/RegStatus/1001> ;
        reg:name                  "donorAgent"@en ;
        rdfs:label                "has donor agent"@en ;
        skos:definition           "Relates an item to an agent who is a former owner of an item who donates the item to another owner."@en ;
        rdf:type                  rdf:Property ;
        rdfs:domain               <http://rdaregistry.info/Elements/c/C10003> ;
        rdfs:subPropertyOf        <http://rdaregistry.info/Elements/i/P40019> ;
        reg:lexicalAlias          <http://rdaregistry.info/Elements/i/donorAgent.en> ;
        reg:hasUnconstrained      <http://rdaregistry.info/Elements/u/P60091> ;
        rdakit:toolkitLabel       "donor agent"@en ;
        rdakit:toolkitDefinition  "An agent who is a former owner of an item who donates the item to another owner."@en ;
        rdfs:label                "a pour agent donateur"@fr ;
        skos:definition           "Met un item en relation avec un ancien agent propriétaire d’un item qui a fait don de cet item à un autre propriétaire."@fr ;
        rdakit:toolkitLabel       "agent donateur"@fr ;
        rdakit:toolkitDefinition  "Ancien agent propriétaire d’un item qui a fait don de cet item à un autre propriétaire."@fr ;
        rdakit:toolkitLabel       "donante"@es ;
        rdakit:toolkitDefinition  "Un propietario anterior de un ítem que lo donó a otro propietario."@es ;
        rdakit:instructionNumber  "18.5" ;
        reg:hasSubproperty        <http://rdaregistry.info/Elements/i/object/P40007> ;
        reg:name                  "ngườiTặng"@vi ;
        rdfs:label                "có người tặng"@vi ;
        skos:definition           "Liên kết bản với người chủ trước đây của bản, người đã tặng bản đó cho người chủ khác."@vi ;
        rdakit:toolkitLabel       "người tặng"@vi ;
        rdakit:toolkitDefinition  "Người chủ trước đây của bản, người đã tặng bản đó cho người chủ khác."@vi ;
        reg:name                  "donor"@da ;
        rdfs:label                "har donor"@da ;
        reg:lexicalAlias          <http://rdaregistry.info/Elements/i/donor.da> ;
        skos:definition           "Relaterer et eksemplar til en tidligere ejer af et eksemplar, der har doneret dette eksemplar til en anden ejer."@da ;
        rdakit:toolkitLabel       "donor"@da ;
        rdakit:toolkitDefinition  "Tidligere ejer af et eksemplar, der har doneret dette eksemplar til en anden ejer."@da ;
        rdfs:label                "hat Stifter"@de ;
        skos:definition           "Setzt ein Exemplar mit einem früheren Eigentümer eines Exemplars, der dieses Exemplar einem anderen Eigentümer überlassen hat, in Beziehung."@de ;
        rdakit:toolkitLabel       "Stifter"@de ;
        rdakit:toolkitDefinition  "Ein früherer Eigentümer eines Exemplars, der dieses Exemplar einem anderen Eigentümer überlassen hat."@de ;
        reg:name                  "δωρητής"@el ;
        rdfs:label                "έχει δωρητή"@el ;
        reg:lexicalAlias          <http://rdaregistry.info/Elements/i/δωρητής.el> ;
        skos:definition           "Συνδέει ένα αντίτυπο με έναν προηγούμενο ιδιοκτήτη ενός αντιτύπου ο οποίος δώρισε αυτό το αντίτυπο σε κάποιον άλλον ιδιοκτήτη."@el ;
        rdakit:toolkitLabel       "δωρητής"@el ;
        rdakit:toolkitDefinition  "Ένας προηγούμενος ιδιοκτήτης ενός αντιτύπου, ο οποίος δώρισε αυτό το αντίτυπο σε κάποιον άλλον ιδιοκτήτη."@el ;
        rdfs:label                "té com a donant"@ca ;
        skos:definition           "Relaciona un item amb un propietari anterior d’un ítem que el va donar a un altre propietari."@ca ;
        rdakit:toolkitLabel       "donant"@ca ;
        rdakit:toolkitDefinition  "Propietari anterior d’un ítem que el va donar a un altre propietari."@ca ;
        reg:name                  "lahjoittaja"@fi ;
        rdfs:label                "lahjoittaja"@fi ;
        reg:lexicalAlias          <rdaa:lahjoittaja.fi> ;
        skos:definition           "Liittää kappaleen sen aikaisempaan omistajaan, joka on lahjoittanut sen toiselle omistajalle."@fi ;
        rdakit:toolkitLabel       "lahjoittaja"@fi ;
        rdakit:toolkitDefinition  "Kappaleen aikaisempi omistaja, joka on lahjoittanut sen toiselle omistajalle."@fi ;
        reg:name                  "donateur"@fr ;
        reg:lexicalAlias          <http://rdaregistry.info/Elements/i/agentDonateur.fr> ;
        rdakit:toolkitLabel       "giver"@no ;
        rdakit:toolkitDefinition  "En tidligere eier av et eksemplar, som har gitt eksemplaret til en annen eier."@no ;
        rdakit:hasElementType     "2" ;
        reg:name                  "adományozó"@hu ;
        rdfs:label                "van adományozója"@hu ;
        skos:definition           "Egy példányt hozzákapcsol egy példány korábbi tulajdonosához, aki a tételt egy másik tulajdonosnak adományozta. "@hu ;
        rdakit:toolkitLabel       "adományozó"@hu ;
        rdakit:toolkitDefinition  "Egy példány korábbi tulajdonosa, aki a példányt egy másik tulajdonosnak adományozta."@hu ;
        skos:altLabel             "donor"@en ;
        skos:altLabel             "donateur"@fr .

<http://rdaregistry.info/Elements/i/P40124>
        rdfs:isDefinedBy          <http://rdaregistry.info/Elements/i/> ;
        reg:status                <http://metadataregistry.org/uri/RegStatus/1001> ;
        rdfs:label                "has donor collective agent"@en ;
        reg:lexicalAlias          <http://rdaregistry.info/Elements/i/donorCollectiveAgent.en> ;
        skos:definition           "Relates an item to a collective agent who is a former owner of an item who donates the item to another owner."@en ;
        rdakit:toolkitLabel       "donor collective agent"@en ;
        rdakit:toolkitDefinition  "A collective agent who is a former owner of an item who donates the item to another owner."@en ;
        rdf:type                  rdf:Property ;
        reg:name                  "donorCollectiveAgent" ;
        rdfs:domain               <http://rdaregistry.info/Elements/c/C10003> ;
        rdakit:hasElementType     "2" ;
        reg:hasSubproperty        <http://rdaregistry.info/Elements/i/datatype/P40124> ;
        reg:hasSubproperty        <http://rdaregistry.info/Elements/i/object/P40124> ;
        rdfs:subPropertyOf        <http://rdaregistry.info/Elements/i/P40118> ;
        rdfs:subPropertyOf        <http://rdaregistry.info/Elements/i/P40007> ;
        reg:hasSubproperty        <http://rdaregistry.info/Elements/i/P40140> ;
        reg:hasSubproperty        <http://rdaregistry.info/Elements/i/P40156> ;
        reg:hasUnconstrained      <http://rdaregistry.info/Elements/u/P60091> ;
        rdfs:label                "a pour agent collectif donateur"@fr ;
        skos:definition           "Met un item en relation avec un ancien agent collectif propriétaire d’un item qui a fait don de cet item à un autre propriétaire."@fr ;
        rdakit:toolkitLabel       "agent collectif donateur"@fr ;
        rdakit:toolkitDefinition  "Ancien agent collectif propriétaire d’un item qui a fait don de cet item à un autre propriétaire."@fr ;
        reg:lexicalAlias          <http://rdaregistry.info/Elements/i/agentCollectifDonateur.fr> .

<http://rdaregistry.info/Elements/i/P40140>
        rdfs:isDefinedBy          <http://rdaregistry.info/Elements/i/> ;
        reg:status                <http://metadataregistry.org/uri/RegStatus/1001> ;
        rdfs:label                "has donor corporate body"@en ;
        reg:lexicalAlias          <http://rdaregistry.info/Elements/i/donorCorporateBody.en> ;
        skos:definition           "Relates an item to a corporate body who is a former owner of an item who donates the item to another owner."@en ;
        rdakit:toolkitLabel       "donor corporate body"@en ;
        rdakit:toolkitDefinition  "A corporate body who is a former owner of an item who donates the item to another owner."@en ;
        rdf:type                  rdf:Property ;
        reg:name                  "donorCorporateBody" ;
        rdfs:domain               <http://rdaregistry.info/Elements/c/C10003> ;
        rdakit:hasElementType     "2" ;
        reg:hasSubproperty        <http://rdaregistry.info/Elements/i/datatype/P40140> ;
        reg:hasSubproperty        <http://rdaregistry.info/Elements/i/object/P40140> ;
        rdfs:subPropertyOf        <http://rdaregistry.info/Elements/i/P40134> ;
        rdfs:subPropertyOf        <http://rdaregistry.info/Elements/i/P40124> ;
        reg:hasUnconstrained      <http://rdaregistry.info/Elements/u/P60091> ;
        rdfs:label                "a pour collectivité donatrice"@fr ;
        skos:definition           "Met un item en relation avec une ancienne collectivité propriétaire d’un item qui a fait don de cet item à un autre propriétaire."@fr ;
        rdakit:toolkitLabel       "collectivité donatrice"@fr ;
        rdakit:toolkitDefinition  "Ancienne collectivité propriétaire d’un item qui a fait don de cet item à un autre propriétaire."@fr ;
        reg:lexicalAlias          <http://rdaregistry.info/Elements/i/collectivitéDonatrice.fr> .

<http://rdaregistry.info/Elements/i/P40156>
        rdfs:isDefinedBy          <http://rdaregistry.info/Elements/i/> ;
        reg:status                <http://metadataregistry.org/uri/RegStatus/1001> ;
        rdfs:label                "has donor family"@en ;
        reg:lexicalAlias          <http://rdaregistry.info/Elements/i/donorFamily.en> ;
        skos:definition           "Relates an item to a family who is a former owner of an item who donates the item to another owner."@en ;
        rdakit:toolkitLabel       "donor family"@en ;
        rdakit:toolkitDefinition  "A family who is a former owner of an item who donates the item to another owner."@en ;
        rdf:type                  rdf:Property ;
        reg:name                  "donorFamily" ;
        rdfs:domain               <http://rdaregistry.info/Elements/c/C10003> ;
        rdakit:hasElementType     "2" ;
        reg:hasSubproperty        <http://rdaregistry.info/Elements/i/datatype/P40156> ;
        reg:hasSubproperty        <http://rdaregistry.info/Elements/i/object/P40156> ;
        rdfs:subPropertyOf        <http://rdaregistry.info/Elements/i/P40150> ;
        rdfs:subPropertyOf        <http://rdaregistry.info/Elements/i/P40124> ;
        reg:hasUnconstrained      <http://rdaregistry.info/Elements/u/P60091> ;
        rdfs:label                "a pour famille donatrice"@fr ;
        skos:definition           "Met un item en relation avec une ancienne famille propriétaire d’un item qui a fait don de cet item à un autre propriétaire."@fr ;
        rdakit:toolkitLabel       "famille donatrice"@fr ;
        rdakit:toolkitDefinition  "Ancienne famille propriétaire d’un item qui a fait don de cet item à un autre propriétaire."@fr ;
        reg:lexicalAlias          <http://rdaregistry.info/Elements/i/familleDonatrice.fr> .

<http://rdaregistry.info/Elements/i/P40108>
        rdfs:isDefinedBy          <http://rdaregistry.info/Elements/i/> ;
        reg:status                <http://metadataregistry.org/uri/RegStatus/1001> ;
        rdfs:label                "has donor person"@en ;
        reg:lexicalAlias          <http://rdaregistry.info/Elements/i/donorPerson.en> ;
        skos:definition           "Relates an item to a person who is a former owner of an item who donates the item to another owner."@en ;
        rdakit:toolkitLabel       "donor person"@en ;
        rdakit:toolkitDefinition  "A person who is a former owner of an item who donates the item to another owner."@en ;
        rdf:type                  rdf:Property ;
        reg:name                  "donorPerson" ;
        rdfs:domain               <http://rdaregistry.info/Elements/c/C10003> ;
        rdakit:hasElementType     "2" ;
        reg:hasSubproperty        <http://rdaregistry.info/Elements/i/datatype/P40108> ;
        reg:hasSubproperty        <http://rdaregistry.info/Elements/i/object/P40108> ;
        rdfs:subPropertyOf        <http://rdaregistry.info/Elements/i/P40102> ;
        rdfs:subPropertyOf        <http://rdaregistry.info/Elements/i/P40007> ;
        reg:hasUnconstrained      <http://rdaregistry.info/Elements/u/P60091> ;
        rdfs:label                "a pour personne donatrice"@fr ;
        skos:definition           "Met un item en relation avec une ancienne personne propriétaire d’un item qui a fait don de cet item à un autre propriétaire."@fr ;
        rdakit:toolkitLabel       "personne donatrice"@fr ;
        rdakit:toolkitDefinition  "Ancienne personne propriétaire d’un item qui a fait don de cet item à un autre propriétaire."@fr ;
        reg:lexicalAlias          <http://rdaregistry.info/Elements/i/personneDonatrice.fr> .

<http://rdaregistry.info/Elements/i/P40057>
        rdfs:isDefinedBy          <http://rdaregistry.info/Elements/i/> ;
        reg:status                <http://metadataregistry.org/uri/RegStatus/1008> ;
        rdf:type                  rdf:Property ;
        rdfs:domain               <http://rdaregistry.info/Elements/c/C10003> ;
        reg:hasUnconstrained      <http://rdaregistry.info/Elements/u/P60083> ;
        rdfs:label                "a pour reproduction électronique (item)"@fr ;
        skos:definition           "Met un item en relation avec un item en format numérique qui résulte du transfert d’un item sur support analogique."@fr ;
        rdakit:toolkitLabel       "reproduction électronique (item)"@fr ;
        rdakit:toolkitDefinition  "Item en format numérique qui résulte du transfert d’un item sur support analogique."@fr ;
        rdakit:toolkitLabel       "reproducción electrónica (ítem)"@es ;
        rdakit:toolkitDefinition  "Un ítem en un formato digital que es el resultado de la transferencia de un ítem en un formato analógico."@es ;
        rdfs:subPropertyOf        <http://rdaregistry.info/Elements/i/P40055> ;
        rdakit:instructionNumber  "24.5" ;
        reg:hasSubproperty        <http://rdaregistry.info/Elements/i/object/P40057> ;
        reg:name                  "bảnSaoChépĐiệnTử"@vi ;
        rdfs:label                "có sao chép điện tử (bản)"@vi ;
        skos:definition           "Liên kết bản với bản dưới định dạng số là kết quả của việc chuyển ạng của bản dưới định dạng tương tự."@vi ;
        rdakit:toolkitLabel       "sao chép điện tử (bản)"@vi ;
        rdakit:toolkitDefinition  "Bản dưới định dạng số là kết quả của việc chuyển ạng của bản dưới định dạng tương tự."@vi ;
        reg:name                  "elektroniskReproduktionEksemplar"@da ;
        rdfs:label                "har elektronisk reproduktion (eksemplar)"@da ;
        reg:lexicalAlias          <http://rdaregistry.info/Elements/i/elektroniskReproduktionEksemplar.da> ;
        skos:definition           "Relaterer et eksemplar til et eksemplar i et digitalt format, der er resultatet af overførsel af et eksemplar i analogt format."@da ;
        rdakit:toolkitLabel       "elektronisk reproduktion (eksemplar)"@da ;
        rdakit:toolkitDefinition  "Eksemplar i et digitalt format, der er resultatet af overførsel af et eksemplar i analogt format."@da ;
        rdfs:label                "hat elektronische Reproduktion (Exemplar)"@de ;
        skos:definition           "Setzt ein Exemplar mit einem Exemplar in einem digitalen Format, das das Ergebnis der Übertragung eines Exemplars in einem analogen Format ist, in Beziehung."@de ;
        rdakit:toolkitLabel       "Elektronische Reproduktion (Exemplar)"@de ;
        rdakit:toolkitDefinition  "Ein Exemplar in einem digitalen Format, das das Ergebnis der Übertragung eines Exemplars in einem analogen Format ist."@de ;
        reg:name                  "ηλεκτρονικήΑναπαραγωγήΑντιτύπου"@el ;
        rdfs:label                "έχει ηλεκτρονική αναπαραγωγή (αντίτυπο)"@el ;
        reg:lexicalAlias          <http://rdaregistry.info/Elements/i/ηλεκτρονικήΑναπαραγωγήΑντιτύπου.el> ;
        skos:definition           "Συνδέει ένα αντίτυπο με ένα αντίτυπο σε ένα ψηφιακό μορφότυπο η οποία προκύπτει από τη μεταφορά ενός αντιτύπου σε αναλογικό μορφότυπο."@el ;
        rdakit:toolkitLabel       "ηλεκτρονική αναπαραγωγή (αντίτυπο)"@el ;
        rdakit:toolkitDefinition  "Ένα αντίτυπο σε ένα ψηφιακό μορφότυπο το οποίο προκύπτει από τη μεταφορά ενός αντιτύπου σε αναλογικό μορφότυπο."@el ;
        rdfs:label                "té com a reproducció electrònica (ítem)"@ca ;
        skos:definition           "Relaciona un item amb un ítem en un format digital que és el resultat de la transferència d’un ítem en format analògic."@ca ;
        rdakit:toolkitLabel       "reproducció electrònica (ítem)"@ca ;
        rdakit:toolkitDefinition  "Ítem en un format digital que és el resultat de la transferència d’un ítem en format analògic."@ca ;
        reg:name                  "digitoitunaKappale"@fi ;
        rdfs:label                "digitoituna (kappale)"@fi ;
        reg:lexicalAlias          <rdaa:digitoitunaKappale.fi> ;
        skos:definition           "Liittää kappaleen digitaalisessa muodossa olevaan kappaleeseen, joka syntyi analogisessa muodossa olevan kappaleen digitoinnin tuloksena."@fi ;
        rdakit:toolkitLabel       "digitoituna (kappale)"@fi ;
        rdakit:toolkitDefinition  "Digitaalisessa muodossa oleva kappale, joka syntyi analogisessa muodossa olevan kappaleen digitoinnin tuloksena."@fi ;
        reg:name                  "reproductionÉlectroniqueItem"@fr ;
        reg:lexicalAlias          <http://rdaregistry.info/Elements/i/reproductionÉlectroniqueItem.fr> ;
        rdakit:toolkitLabel       "elektronisk reproduksjon (eksemplar)"@no ;
        rdakit:toolkitDefinition  "Et eksemplar i digitalt format som er resultatet av overføring av et eksemplar fra analogt format."@no ;
        reg:hasSubproperty        <http://rdaregistry.info/Elements/i/datatype/P40057> .

<http://rdaregistry.info/Elements/i/P40088>
        rdfs:isDefinedBy          <http://rdaregistry.info/Elements/i/> ;
        reg:status                <http://metadataregistry.org/uri/RegStatus/1001> ;
        rdfs:label                "has electronic reproduction of item"@en ;
        rdf:type                  rdf:Property ;
        reg:name                  "electronicReproductionOfItem"@en ;
        reg:lexicalAlias          <http://rdaregistry.info/Elements/i/electronicReproductionOfItem.en> ;
        skos:definition           "Relates an item to a manifestation in a digital format that is the result of the transfer of an item in analog format."@en ;
        rdfs:domain               <http://rdaregistry.info/Elements/c/C10003> ;
        rdfs:subPropertyOf        <http://rdaregistry.info/Elements/i/P40092> ;
        rdakit:toolkitLabel       "electronic reproduction of item"@en ;
        rdakit:toolkitDefinition  "A manifestation in a digital format that is the result of the transfer of an item in analog format."@en ;
        reg:hasUnconstrained      <http://rdaregistry.info/Elements/u/P60083> ;
        rdakit:hasElementType     "2" ;
        reg:hasSubproperty        <http://rdaregistry.info/Elements/i/datatype/P40088> ;
        rdfs:label                "a pour reproduction électronique d’un item"@fr ;
        skos:definition           "Met un item en relation avec une manifestation en format numérique qui est le résultat du transfert d’un item sur support analogique."@fr ;
        rdakit:toolkitLabel       "reproduction électronique d’un item"@fr ;
        rdakit:toolkitDefinition  "Manifestation en format numérique qui est le résultat du transfert d’un item sur support analogique."@fr ;
        reg:lexicalAlias          <http://rdaregistry.info/Elements/i/reproductionÉlectroniqueDunItem.fr> ;
        skos:altLabel             "electronic reproduction (item)"@en .

<http://rdaregistry.info/Elements/i/P40027>
        rdfs:isDefinedBy          <http://rdaregistry.info/Elements/i/> ;
        reg:status                <http://metadataregistry.org/uri/RegStatus/1008> ;
        rdf:type                  rdf:Property ;
        rdfs:domain               <http://rdaregistry.info/Elements/c/C10003> ;
        rdfs:subPropertyOf        <http://rdaregistry.info/Elements/i/P40042> ;
        reg:hasUnconstrained      <http://rdaregistry.info/Elements/u/P60469> ;
        rdfs:label                "est une reproduction électronique de (item)"@fr ;
        skos:definition           "Met un item en relation avec un item sur support analogique qui a été transféré dans un format numérique."@fr ;
        rdakit:toolkitLabel       "reproduction électronique de (item)"@fr ;
        rdakit:toolkitDefinition  "Item sur support analogique qui a été transféré dans un format numérique."@fr ;
        rdakit:toolkitLabel       "reproducción electrónica (ítem)"@es ;
        rdakit:toolkitDefinition  "Un ítem en un formato digital que es el resultado de la transferencia de un ítem en un formato analógico."@es ;
        rdakit:instructionNumber  "24.5" ;
        reg:hasSubproperty        <http://rdaregistry.info/Elements/i/object/P40027> ;
        reg:name                  "phiênBảnĐiệnTửCủaBản"@vi ;
        rdfs:label                "là phiên bản điện tử của (bản)"@vi ;
        skos:definition           "Liên kết bản với bản dưới định dạng tương tự được chuyển sang định dạng số"@vi ;
        rdakit:toolkitLabel       "phiên bản điện tử của (bản)"@vi ;
        rdakit:toolkitDefinition  "Bản dưới định dạng tương tự được chuyển sang định dạng số"@vi ;
        reg:name                  "elektroniskReproduktionAfEksemplar"@da ;
        rdfs:label                "er elektronisk reproduktion af (eksemplar)"@da ;
        reg:lexicalAlias          <http://rdaregistry.info/Elements/i/elektroniskReproduktionAfEksemplar.da> ;
        skos:definition           "Relaterer et eksemplar til et eksemplar i et analogt format, der er overført til et digitalt format."@da ;
        rdakit:toolkitLabel       "elektronisk reproduktion af (eksemplar)"@da ;
        rdakit:toolkitDefinition  "Eksemplar i et analogt format, der er overført til et digitalt format."@da ;
        rdfs:label                "ist elektronische Reproduktion von (Exemplar)"@de ;
        skos:definition           "Setzt ein Exemplar mit einem Exemplar in einem analogen Format, das in ein digitales Format übertragen wurde, in Beziehung."@de ;
        rdakit:toolkitLabel       "Elektronische Reproduktion von (Exemplar)"@de ;
        rdakit:toolkitDefinition  "Ein Exemplar in einem analogen Format, das in ein digitales Format übertragen wurde."@de ;
        reg:name                  "ηλεκτρονικήΑναπαραγωγήΤουΑντιτύπου"@el ;
        rdfs:label                "είναι ηλεκτρονική αναπαραγωγή του (αντίτυπο)"@el ;
        reg:lexicalAlias          <http://rdaregistry.info/Elements/i/ηλεκτρονικήΑναπαραγωγήΤουΑντιτύπου.el> ;
        skos:definition           "Συνδέει ένα αντίτυπο με ένα αντίτυπο σε ένα αναλογικό μορφότυπο το οποίο μεταφέρεται σε ένα ψηφιακό μορφότυπο."@el ;
        rdakit:toolkitLabel       "ηλεκτρονική αναπαραγωγή του (αντίτυπο)"@el ;
        rdakit:toolkitDefinition  "Ένα αντίτυπο σε ένα αναλογικό μορφότυπο το οποίο μεταφέρεται σε ένα ψηφιακό μορφότυπο."@el ;
        rdfs:label                "és reproducció electrònica de (ítem)"@ca ;
        skos:definition           "Relaciona un item amb un ítem en un format analògic que es transfereix a un format digital."@ca ;
        rdakit:toolkitLabel       "reproducció electrònica de (ítem)"@ca ;
        rdakit:toolkitDefinition  "Ítem en un format analògic que es transfereix a un format digital."@ca ;
        reg:name                  "digitoituKappaleesta"@fi ;
        rdfs:label                "digitoitu kappaleesta"@fi ;
        reg:lexicalAlias          <rdaa:digitoituKappaleesta.fi> ;
        skos:definition           "Liittää kappaleen analogisessa muodossa olevaan kappaleeseen, josta kuvailun kohde on digitoitu."@fi ;
        rdakit:toolkitLabel       "digitoitu kappaleesta"@fi ;
        rdakit:toolkitDefinition  "Analogisessa muodossa oleva kappale, joka on muunnettu digitaaliseen muotoon."@fi ;
        reg:name                  "reproductionÉlectroniqueDeItem"@fr ;
        reg:lexicalAlias          <http://rdaregistry.info/Elements/i/reproductionÉlectroniqueDeItem.fr> ;
        rdakit:toolkitLabel       "elektronisk reproduksjon av (eksemplar)"@no ;
        rdakit:toolkitDefinition  "Et eksemplar i et analogt format som overføres til et digitalt format."@no ;
        reg:hasSubproperty        <http://rdaregistry.info/Elements/i/datatype/P40027> .

<http://rdaregistry.info/Elements/i/P40031>
        rdfs:isDefinedBy          <http://rdaregistry.info/Elements/i/> ;
        reg:status                <http://metadataregistry.org/uri/RegStatus/1001> ;
        reg:name                  "equivalentItem"@en ;
        rdfs:label                "has equivalent item"@en ;
        skos:definition           "Relates an item to an item that exemplifies a manifestation that embodies the same expression of a work."@en ;
        rdf:type                  rdf:Property ;
        rdfs:domain               <http://rdaregistry.info/Elements/c/C10003> ;
        rdfs:subPropertyOf        <http://rdaregistry.info/Elements/i/P40046> ;
        reg:hasSubproperty        <http://rdaregistry.info/Elements/i/P40042> ;
        reg:lexicalAlias          <http://rdaregistry.info/Elements/i/equivalentItem.en> ;
        reg:hasUnconstrained      <http://rdaregistry.info/Elements/u/P60191> ;
        rdakit:toolkitLabel       "equivalent item"@en ;
        rdakit:toolkitDefinition  "An item that exemplifies a manifestation that embodies the same expression of a work."@en ;
        rdfs:label                "a pour item équivalent"@fr ;
        skos:definition           "Met un item en relation avec un item qui représente une manifestation matérialisant la même expression d’une œuvre."@fr ;
        rdakit:toolkitLabel       "item équivalent"@fr ;
        rdakit:toolkitDefinition  "Item qui représente une manifestation matérialisant la même expression d’une œuvre."@fr ;
        rdakit:toolkitLabel       "equivalente (ítem)"@es ;
        rdakit:toolkitDefinition  "Un ítem que ejemplifica una manifestación que materializa la misma expresión de una obra."@es ;
        reg:hasSubproperty        <http://rdaregistry.info/Elements/i/P40055> ;
        rdakit:instructionNumber  "24.5" ;
        reg:hasSubproperty        <http://rdaregistry.info/Elements/i/object/P40031> ;
        reg:name                  "bảnTươngĐương"@vi ;
        rdfs:label                "là tương đương (bản)"@vi ;
        skos:definition           "Liên kết bản với thể hiện biểu thị là hiện thấn của cùng biểu hiện của tác phẩm."@vi ;
        rdakit:toolkitLabel       "tương đương (bản)"@vi ;
        rdakit:toolkitDefinition  "Thể hiện biểu thị là hiện thấn của cùng biểu hiện của tác phẩm."@vi ;
        reg:name                  "ækvivalentEksemplar"@da ;
        rdfs:label                "har ækvivalent (eksemplar)"@da ;
        reg:lexicalAlias          <http://rdaregistry.info/Elements/i/ækvivalentEksemplar.da> ;
        skos:definition           "Relaterer et eksemplar til et eksemplar, der eksemplificerer en manifestation, som omfatter det samme udtryk af et værk."@da ;
        rdakit:toolkitLabel       "ækvivalent (eksemplar)"@da ;
        rdakit:toolkitDefinition  "Eksemplar, der eksemplificerer en manifestation, som omfatter det samme udtryk af et værk."@da ;
        rdfs:label                "hat Äquivalent (Exemplar)"@de ;
        skos:definition           "Setzt ein Exemplar mit einem Exemplar, das eine Manifestation darstellt, das dieselbe Expression eines Werks verkörpert, in Beziehung."@de ;
        rdakit:toolkitLabel       "Äquivalent (Exemplar)"@de ;
        rdakit:toolkitDefinition  "Ein Exemplar, das eine Manifestation darstellt, das dieselbe Expression eines Werks verkörpert."@de ;
        reg:name                  "ισοδύναμοΑντίτυπο"@el ;
        rdfs:label                "είναι ισοδύναμο (αντίτυπο)"@el ;
        reg:lexicalAlias          <http://rdaregistry.info/Elements/i/ισοδύναμοΑντίτυπο.el> ;
        skos:definition           "Συνδέει ένα αντίτυπο με ένα αντίτυπο το οποίο αποτελεί παράδειγμα υλοποίησης μιας εκδήλωσης που ενσωματώνει την ίδια έκφραση ενός έργου."@el ;
        rdakit:toolkitLabel       "ισοδύναμο (αντίτυπο)"@el ;
        rdakit:toolkitDefinition  "Ένα αντίτυπο το οποίο αποτελεί παράδειγμα υλοποίησης μιας εκδήλωσης που ενσωματώνει την ίδια έκφραση ενός έργου."@el ;
        rdfs:label                "és ítem equivalent"@ca ;
        skos:definition           "Relaciona un item amb un ítem que exemplifica una manifestació que materialitza la mateixa expressió d’una obra."@ca ;
        rdakit:toolkitLabel       "ítem equivalent"@ca ;
        rdakit:toolkitDefinition  "Ítem que exemplifica una manifestació que materialitza la mateixa expressió d’una obra."@ca ;
        reg:name                  "vastaavaKappale"@fi ;
        rdfs:label                "vastaava kappale"@fi ;
        reg:lexicalAlias          <rdaa:vastaavaKappale.fi> ;
        skos:definition           "Liittää kappaleen kappaleeseen, joka edustaa saman ekspression manifestaatiota."@fi ;
        rdakit:toolkitLabel       "vastaava kappale"@fi ;
        rdakit:toolkitDefinition  "Kappale, joka edustaa teoksen saman ekspression manifestaatiota."@fi ;
        reg:name                  "équivalentItem"@fr ;
        reg:lexicalAlias          <http://rdaregistry.info/Elements/i/itemÉquivalent.fr> ;
        rdakit:toolkitLabel       "ekvivalent (eksemplar)"@no ;
        rdakit:toolkitDefinition  "Et eksemplar som er et eksempel på en manifestasjon som legemliggjør det samme uttrykket av et verk."@no ;
        rdakit:hasElementType     "3" ;
        reg:name                  "egyenértékűPéldány"@hu ;
        rdfs:label                "egyenértékű (példány)"@hu ;
        skos:definition           "Egy példányt hozzákapcsol egy olyan példányhoz, amely egy megjelenési formát példáz, amely egy mű ugyanazon kifejezési formáját testesíti meg."@hu ;
        rdakit:toolkitLabel       "egyenértékű (példány)"@hu ;
        rdakit:toolkitDefinition  "Egy példány, amely egy megjelenési formát példáz, amely egy mű ugyanazon kifejezési formáját testesíti meg."@hu ;
        skos:altLabel             "equivalent item relationship"@en .

<http://rdaregistry.info/Elements/i/P40053>
        rdfs:isDefinedBy          <http://rdaregistry.info/Elements/i/> ;
        reg:status                <http://metadataregistry.org/uri/RegStatus/1008> ;
        reg:name                  "equivalentItemRelationship"@en ;
        rdf:type                  rdf:Property ;
        rdfs:domain               <http://rdaregistry.info/Elements/c/C10003> ;
        rdfs:subPropertyOf        <http://rdaregistry.info/Elements/i/P40046> ;
        reg:hasSubproperty        <http://rdaregistry.info/Elements/i/P40031> ;
        reg:lexicalAlias          <http://rdaregistry.info/Elements/i/equivalentItemRelationship.en> ;
        reg:hasUnconstrained      <http://rdaregistry.info/Elements/u/P60712> ;
        rdfs:label                "a pour relation d’item équivalent"@fr ;
        skos:definition           "Met un item en relation avec un item qui est équivalent à un autre item."@fr ;
        rdakit:toolkitLabel       "relation d’item équivalent"@fr ;
        rdakit:toolkitDefinition  "Item qui est équivalent à un autre item."@fr ;
        rdakit:toolkitLabel       "relaciones de ítem equivalente"@es ;
        rdakit:toolkitDefinition  "Un ítem que es equivalente al ítem."@es ;
        rdakit:instructionNumber  "18.5" ;
        reg:hasSubproperty        <http://rdaregistry.info/Elements/i/object/P40053> ;
        reg:name                  "mốiQuanHệBảnTươngĐương"@vi ;
        rdfs:label                "có mối quan hệ bản tương đương với"@vi ;
        skos:definition           "Liên kết bản với bản tương đương với bản khác."@vi ;
        rdakit:toolkitLabel       "mối quan hệ bản tương đương"@vi ;
        rdakit:toolkitDefinition  "Bản tương đương với bản khác."@vi ;
        reg:name                  "ækvivalentEksemplarrelation"@da ;
        rdfs:label                "har ækvivalent eksemplarrelation med"@da ;
        reg:lexicalAlias          <http://rdaregistry.info/Elements/i/ækvivalentEksemplarrelation.da> ;
        skos:definition           "Relaterer et eksemplar til et eksemplar der er ækvivalent til et eksemplar."@da ;
        rdakit:toolkitLabel       "ækvivalent eksemplarrelation"@da ;
        rdakit:toolkitDefinition  "Eksemplar der er ækvivalent til et eksemplar."@da ;
        rdfs:label                "hat Äquivalenzbeziehung auf Exemplarebene"@de ;
        skos:definition           "Setzt ein Exemplar mit einem Exemplar, das mit einem anderen Exemplar äquivalent ist, in Beziehung."@de ;
        rdakit:toolkitLabel       "Äquivalenzbeziehung auf Exemplarebene"@de ;
        rdakit:toolkitDefinition  "Ein Exemplar, das mit einem anderen Exemplar äquivalent ist."@de ;
        reg:name                  "ισοδύναμηΣχέσηΑντιτύπου"@el ;
        rdfs:label                "έχει ισοδύναμη σχέση του αντιτύπου με"@el ;
        reg:lexicalAlias          <http://rdaregistry.info/Elements/i/ισοδύναμηΣχέσηΑντιτύπου.el> ;
        skos:definition           "Συνδέει ένα αντίτυπο με ένα αντίτυπο το οποίο είναι ισοδύναμο με κάποιο άλλο αντίτυπο."@el ;
        rdakit:toolkitLabel       "ισοδύναμη σχέση του αντιτύπου"@el ;
        rdakit:toolkitDefinition  "Ένα αντίτυπο το οποίο είναι ισοδύναμο με κάποιο άλλο αντίτυπο."@el ;
        rdfs:label                "té com a relació d’ítem equivalent"@ca ;
        skos:definition           "Relaciona un item amb un ítem que és equivalent a un altre ítem."@ca ;
        rdakit:toolkitLabel       "relació d’ítem equivalent"@ca ;
        rdakit:toolkitDefinition  "Ítem que és equivalent a un altre ítem."@ca ;
        reg:name                  "suhdeVastaavaanKappaleeseen"@fi ;
        rdfs:label                "suhde vastaavaan kappaleeseen"@fi ;
        reg:lexicalAlias          <rdaa:suhdeVastaavaanKappaleeseen.fi> ;
        skos:definition           "Liittää kappaleen kappaleeseen, joka vastaa toista kappaletta."@fi ;
        rdakit:toolkitLabel       "suhde vastaavaan kappaleeseen"@fi ;
        rdakit:toolkitDefinition  "Kappale, joka vastaa toista kappaletta."@fi ;
        reg:name                  "relationDitemÉquivalent"@fr ;
        reg:lexicalAlias          <http://rdaregistry.info/Elements/i/relationDitemÉquivalent.fr> ;
        rdakit:toolkitLabel       "ekvivalent eksemplar: relasjonstype"@no ;
        rdakit:toolkitDefinition  "Et eksemplar som tilsvarer et annet eksemplar."@no ;
        reg:hasSubproperty        <http://rdaregistry.info/Elements/i/datatype/P40053> .

<http://rdaregistry.info/Elements/i/P40037>
        rdfs:isDefinedBy    <http://rdaregistry.info/Elements/i/> ;
        reg:status          <http://metadataregistry.org/uri/RegStatus/1008> ;
        rdf:type            rdf:Property ;
        rdfs:subPropertyOf  <http://rdaregistry.info/Elements/i/P40030> .

<http://rdaregistry.info/Elements/i/P40058>
        rdfs:isDefinedBy          <http://rdaregistry.info/Elements/i/> ;
        reg:status                <http://metadataregistry.org/uri/RegStatus/1008> ;
        rdf:type                  rdf:Property ;
        rdfs:domain               <http://rdaregistry.info/Elements/c/C10003> ;
        reg:hasUnconstrained      <http://rdaregistry.info/Elements/u/P60217> ;
        rdfs:label                "a pour fac-similé (item)"@fr ;
        skos:definition           "Met un item en relation avec un item qui reproduit exactement un autre item."@fr ;
        rdakit:toolkitLabel       "fac-similé (item)"@fr ;
        rdakit:toolkitDefinition  "Item qui reproduit exactement un autre item."@fr ;
        rdakit:toolkitLabel       "facsímil (ítem)"@es ;
        rdakit:toolkitDefinition  "Un ítem que reproduce exactamente un ítem."@es ;
        rdfs:subPropertyOf        <http://rdaregistry.info/Elements/i/P40055> ;
        reg:hasSubproperty        <http://rdaregistry.info/Elements/i/P40059> ;
        rdakit:instructionNumber  "24.5" ;
        reg:hasSubproperty        <http://rdaregistry.info/Elements/i/object/P40058> ;
        reg:name                  "bảnSaoChép"@vi ;
        rdfs:label                "có sao chép (bản)"@vi ;
        skos:definition           "Liên kết bản với bản tạo lại chính xác bản khác."@vi ;
        rdakit:toolkitLabel       "sao chép (bản)"@vi ;
        rdakit:toolkitDefinition  "Bản tạo lại chính xác bản khác."@vi ;
        reg:name                  "faksimileEksemplar"@da ;
        rdfs:label                "har faksimile (eksemplar)"@da ;
        reg:lexicalAlias          <http://rdaregistry.info/Elements/i/faksimileEksemplar.da> ;
        skos:definition           "Relaterer et eksemplar til et eksemplar, der er en nøjagtig reproduktion af et andet eksemplar."@da ;
        rdakit:toolkitLabel       "faksimile (eksemplar)"@da ;
        rdakit:toolkitDefinition  "Eksemplar, der er en nøjagtig reproduktion af et andet eksemplar."@da ;
        rdfs:label                "hat Faksimile (Exemplar)"@de ;
        skos:definition           "Setzt ein Exemplar mit einem Exemplar, das ein anderes Exemplar exakt reproduziert, in Beziehung."@de ;
        rdakit:toolkitLabel       "Faksimile (Exemplar)"@de ;
        rdakit:toolkitDefinition  "Ein Exemplar, das ein anderes Exemplar exakt reproduziert."@de ;
        reg:name                  "ομοιότυποΑντίτυπο"@el ;
        rdfs:label                "έχει ομοιότυπο (αντίτυπο)"@el ;
        reg:lexicalAlias          <http://rdaregistry.info/Elements/i/ομοιότυποΑντίτυπο.el> ;
        skos:definition           "Συνδέει ένα αντίτυπο με ένα αντίτυπο το οποίο αναπαράγει ακριβώς κάποιο άλλο αντίτυπο."@el ;
        rdakit:toolkitLabel       "ομοιότυπο (αντίτυπο)"@el ;
        rdakit:toolkitDefinition  "Ένα αντίτυπο το οποίο αναπαράγει ακριβώς κάποιο άλλο αντίτυπο."@el ;
        rdfs:label                "té com a facsímil (ítem)"@ca ;
        skos:definition           "Relaciona un item amb un ítem que reprodueix exactament un ítem."@ca ;
        rdakit:toolkitLabel       "facsímil (ítem)"@ca ;
        rdakit:toolkitDefinition  "Ítem que reprodueix exactament un ítem."@ca ;
        reg:name                  "nakoispainosKappale"@fi ;
        rdfs:label                "näköispainos (kappale)"@fi ;
        reg:lexicalAlias          <rdaa:nakoispainosKappale.fi> ;
        skos:definition           "Liittää kappaleen kappaleeseen, joka on toisen kappaleen täysin identtinen jäljennös."@fi ;
        rdakit:toolkitLabel       "näköispainos (kappale)"@fi ;
        rdakit:toolkitDefinition  "Kappale, joka on toisen kappaleen täysin identtinen jäljennös."@fi ;
        reg:name                  "facsimiléItem"@fr ;
        reg:lexicalAlias          <http://rdaregistry.info/Elements/i/facsimiléItem.fr> ;
        rdakit:toolkitLabel       "faksimile (eksemplar)"@no ;
        rdakit:toolkitDefinition  "Et eksemplar som er en tro kopi av et annet eksemplar."@no ;
        reg:hasSubproperty        <http://rdaregistry.info/Elements/i/datatype/P40058> .

<http://rdaregistry.info/Elements/i/P40089>
        rdfs:isDefinedBy          <http://rdaregistry.info/Elements/i/> ;
        reg:status                <http://metadataregistry.org/uri/RegStatus/1001> ;
        rdfs:label                "has facsimile of item"@en ;
        rdf:type                  rdf:Property ;
        reg:name                  "facsimileOfItem"@en ;
        reg:lexicalAlias          <http://rdaregistry.info/Elements/i/facsimileOfItem.en> ;
        skos:definition           "Relates an item to a manifestation that exactly reproduces an item that exemplifies another manifestation."@en ;
        rdfs:domain               <http://rdaregistry.info/Elements/c/C10003> ;
        rdfs:subPropertyOf        <http://rdaregistry.info/Elements/i/P40092> ;
        rdakit:toolkitLabel       "facsimile of item"@en ;
        rdakit:toolkitDefinition  "A manifestation that exactly reproduces an item that exemplifies another manifestation."@en ;
        reg:hasUnconstrained      <http://rdaregistry.info/Elements/u/P60217> ;
        rdakit:hasElementType     "2" ;
        reg:hasSubproperty        <http://rdaregistry.info/Elements/i/datatype/P40089> ;
        reg:hasSubproperty        <http://rdaregistry.info/Elements/i/P40090> ;
        rdfs:label                "a pour fac-similé d’un item"@fr ;
        skos:definition           "Met un item en relation avec une manifestation qui reproduit exactement un item représentant une autre manifestation."@fr ;
        rdakit:toolkitLabel       "fac-similé d’un item"@fr ;
        rdakit:toolkitDefinition  "Manifestation qui reproduit exactement un item représentant une autre manifestation."@fr ;
        reg:lexicalAlias          <http://rdaregistry.info/Elements/i/facsimiléDunItem.fr> ;
        skos:altLabel             "facsimile (item)"@en .

<http://rdaregistry.info/Elements/i/P40045>
        rdfs:isDefinedBy          <http://rdaregistry.info/Elements/i/> ;
        reg:status                <http://metadataregistry.org/uri/RegStatus/1008> ;
        rdf:type                  rdf:Property ;
        rdfs:domain               <http://rdaregistry.info/Elements/c/C10003> ;
        rdfs:subPropertyOf        <http://rdaregistry.info/Elements/i/P40042> ;
        reg:hasSubproperty        <http://rdaregistry.info/Elements/i/P40044> ;
        reg:hasUnconstrained      <http://rdaregistry.info/Elements/u/P60301> ;
        rdfs:label                "est un fac-un similé de (item)"@fr ;
        skos:definition           "Met un item en relation avec un item qui sert de base à une reproduction exacte."@fr ;
        rdakit:toolkitLabel       "fac-similé de (item)"@fr ;
        rdakit:toolkitDefinition  "Item qui sert de base à une reproduction exacte."@fr ;
        rdakit:toolkitLabel       "facsímil de (ítem)"@es ;
        rdakit:toolkitDefinition  "Un ítem utilizado como base para una reproducción exacta."@es ;
        rdakit:instructionNumber  "24.5" ;
        reg:hasSubproperty        <http://rdaregistry.info/Elements/i/object/P40045> ;
        reg:name                  "bảnSaoCủaBản"@vi ;
        rdfs:label                "là bản sao của (bản)"@vi ;
        skos:definition           "Liên kết bản với bản được sử dụng như là cơ sở cho sản xuất lại chính xác."@vi ;
        rdakit:toolkitLabel       "bản sao của (bản)"@vi ;
        rdakit:toolkitDefinition  "Bản được sử dụng như là cơ sở cho sản xuất lại chính xác."@vi ;
        reg:name                  "faksimileAfEksemplar"@da ;
        rdfs:label                "er faksimile af (eksemplar)"@da ;
        reg:lexicalAlias          <http://rdaregistry.info/Elements/i/faksimileAfEksemplar.da> ;
        skos:definition           "Relaterer et eksemplar til et eksemplar, der er anvendt som grundlag for en nøjagtig reproduktion."@da ;
        rdakit:toolkitLabel       "faksimile af (eksemplar)"@da ;
        rdakit:toolkitDefinition  "Eksemplar, der er anvendt som grundlag for en nøjagtig reproduktion."@da ;
        rdfs:label                "ist Faksimile von (Exemplar)"@de ;
        skos:definition           "Setzt ein Exemplar mit einem Exemplar, das als Grundlage für eine exakte Reproduktion verwendet wurde, in Beziehung."@de ;
        rdakit:toolkitLabel       "Faksimile von (Exemplar)"@de ;
        rdakit:toolkitDefinition  "Ein Exemplar, das als Grundlage für eine exakte Reproduktion verwendet wurde."@de ;
        reg:name                  "ομοιότυποΤουΑντιτύπου"@el ;
        rdfs:label                "είναι ομοιότυπο του (αντίτυπο)"@el ;
        reg:lexicalAlias          <http://rdaregistry.info/Elements/i/ομοιότυποΤουΑντιτύπου.el> ;
        skos:definition           "Συνδέει ένα αντίτυπο με ένα αντίτυπο το οποίο χρησιμοποιείται ως η βάση για μια αναπαραγωγή ακριβείας."@el ;
        rdakit:toolkitLabel       "ομοιότυπο του (αντίτυπο)"@el ;
        rdakit:toolkitDefinition  "Ένα αντίτυπο το οποίο χρησιμοποιείται ως η βάση για μια αναπαραγωγή ακριβείας."@el ;
        rdfs:label                "és facsímil de (ítem)"@ca ;
        skos:definition           "Relaciona un item amb un ítem que s’usa com a base d’una reproducció exacta."@ca ;
        rdakit:toolkitLabel       "facsímil de (ítem)"@ca ;
        rdakit:toolkitDefinition  "Ítem que s’usa com a base d’una reproducció exacta."@ca ;
        reg:name                  "nakoispainoksenAlkuperaKappale"@fi ;
        rdfs:label                "näköispainoksen alkuperä (kappale)"@fi ;
        reg:lexicalAlias          <rdaa:nakoispainoksenAlkuperaKappale.fi> ;
        skos:definition           "Liittää kappaleen kappaleeseen, jota on käytetty täysin identtisen jäljennöksen perustana."@fi ;
        rdakit:toolkitLabel       "näköispainoksen alkuperä (kappale)"@fi ;
        rdakit:toolkitDefinition  "Kappale, jota on käytetty täysin identtisen jäljennöksen perustana."@fi ;
        reg:name                  "facsimiléDeItem"@fr ;
        reg:lexicalAlias          <http://rdaregistry.info/Elements/i/facsimiléDeItem.fr> ;
        rdakit:toolkitLabel       "faksimile av (eksemplar)"@no ;
        rdakit:toolkitDefinition  "Et eksemplar som brukes som utgangspunkt for en eksakt reproduksjon."@no ;
        reg:hasSubproperty        <http://rdaregistry.info/Elements/i/datatype/P40045> .

<http://rdaregistry.info/Elements/i/P40036>
        rdfs:isDefinedBy          <http://rdaregistry.info/Elements/i/> ;
        reg:status                <http://metadataregistry.org/uri/RegStatus/1001> ;
        reg:name                  "filmedWithItem"@en ;
        rdfs:label                "is filmed with item"@en ;
        skos:definition           "Relates an item to an item that is contained on the same microform as an item."@en ;
        rdf:type                  rdf:Property ;
        rdfs:domain               <http://rdaregistry.info/Elements/c/C10003> ;
        rdfs:subPropertyOf        <http://rdaregistry.info/Elements/i/P40029> ;
        reg:lexicalAlias          <http://rdaregistry.info/Elements/i/filmedWithItem.en> ;
        reg:hasUnconstrained      <http://rdaregistry.info/Elements/u/P60258> ;
        rdakit:toolkitLabel       "filmed with item"@en ;
        rdakit:toolkitDefinition  "An item that is contained on the same microform as an item."@en ;
        rdfs:label                "est filmé avec un item"@fr ;
        skos:definition           "Met un item en relation avec un item qui est contenu sur la même microforme qu’un item."@fr ;
        rdakit:toolkitLabel       "filmé avec un item"@fr ;
        rdakit:toolkitDefinition  "Item qui est contenu sur la même microforme qu’un item."@fr ;
        rdakit:toolkitLabel       "filmado con (ítem)"@es ;
        rdakit:toolkitDefinition  "Un ítem que se incluye en la misma microforma que el ítem descrito."@es ;
        rdakit:instructionNumber  "24.5" ;
        reg:hasSubproperty        <http://rdaregistry.info/Elements/i/object/P40036> ;
        reg:name                  "đượcLàmPhimVớiBản"@vi ;
        rdfs:label                "được làm phim với (bản)"@vi ;
        skos:definition           "Liên kết bản với bản được chứa trên cùng vi phim với bản đang được mô tả."@vi ;
        rdakit:toolkitLabel       "được làm phim với (bản)"@vi ;
        rdakit:toolkitDefinition  "Bản được chứa trên cùng vi phim với bản đang được mô tả."@vi ;
        reg:name                  "optagetSammenMedEksemplar"@da ;
        rdfs:label                "er optaget sammen med (eksemplar)"@da ;
        reg:lexicalAlias          <http://rdaregistry.info/Elements/i/optagetSammenMedEksemplar.da> ;
        skos:definition           "Relaterer et eksemplar til et eksemplar, der er indeholdt på én mikroform sammen med det eksemplar, der beskrives."@da ;
        rdakit:toolkitLabel       "optaget sammen med (eksemplar)"@da ;
        rdakit:toolkitDefinition  "Eksemplar, der er indeholdt på én mikroform sammen med det eksemplar, der beskrives."@da ;
        rdfs:label                "ist verfilmt mit (Exemplar)"@de ;
        skos:definition           "Setzt ein Exemplar mit einem Exemplar, das auf derselben Mikroform enthalten ist, wie ein Exemplar, das beschrieben wird, in Beziehung."@de ;
        rdakit:toolkitLabel       "Verfilmt mit (Exemplar)"@de ;
        rdakit:toolkitDefinition  "Ein Exemplar, das auf derselben Mikroform enthalten ist, wie ein Exemplar, das beschrieben wird."@de ;
        reg:name                  "κινηματογραφημένοΜαζίΜεΑντίτυπο"@el ;
        rdfs:label                "είναι κινηματογραφημένο μαζί με (αντίτυπο)"@el ;
        reg:lexicalAlias          <http://rdaregistry.info/Elements/i/κινηματογραφημένοΜαζίΜεΑντίτυπο.el> ;
        skos:definition           "Συνδέει ένα αντίτυπο με ένα αντίτυπο το οποίο περιέχεται στην ίδια μικροφόρμα με ένα περιγραφόμενο αντίτυπο."@el ;
        rdakit:toolkitLabel       "κινηματογραφημένο μαζί με (αντίτυπο)"@el ;
        rdakit:toolkitDefinition  "Ένα αντίτυπο το οποίο περιέχεται στην ίδια μικροφόρμα με ένα περιγραφόμενο αντίτυπο."@el ;
        rdfs:label                "és filmat amb (ítem)"@ca ;
        skos:definition           "Relaciona un item amb un ítem inclòs en la mateixa microforma amb un ítem que es descriu."@ca ;
        rdakit:toolkitLabel       "filmat amb (ítem)"@ca ;
        rdakit:toolkitDefinition  "Ítem inclòs en la mateixa microforma amb un ítem que es descriu."@ca ;
        reg:name                  "mikrofilmillaMyosKappale"@fi ;
        rdfs:label                "mikrofilmillä myös (kappale)"@fi ;
        reg:lexicalAlias          <rdaa:mikrofilmillaMyosKappale.fi> ;
        skos:definition           "Liittää kappaleen kappaleeseen, joka on samalla mikromuotoisella tallenteella kuin kuvailtava kappale."@fi ;
        rdakit:toolkitLabel       "mikrofilmillä myös (kappale)"@fi ;
        rdakit:toolkitDefinition  "Kappale, joka on samalla mikromuotoisella tallenteella kuin kuvailtava kappale."@fi ;
        reg:name                  "filméAvecItem"@fr ;
        reg:lexicalAlias          <http://rdaregistry.info/Elements/i/filméAvecUnItem.fr> ;
        rdakit:toolkitLabel       "på film med (eksemplar)"@no ;
        rdakit:toolkitDefinition  "Et eksemplar som befinner seg på samme mikroform som eksemplaret som beskrives."@no ;
        rdakit:hasElementType     "2" ;
        reg:name                  "Példánnyalfilmezve"@hu ;
        rdfs:label                "filmezve (példány)"@hu ;
        skos:definition           "Egy példányt hozzákapcsol egy olyan példányhoz, amelyet ugyanaz a mikroformátum tartalmaz, mint az éppen leírt példányt."@hu ;
        rdakit:toolkitLabel       "filmezve (példány)"@hu ;
        rdakit:toolkitDefinition  "Egy példány, amely egy éppen leírt példánnyal közös mikroformátumon van."@hu .

<http://rdaregistry.info/Elements/i/P40019>
        rdfs:isDefinedBy          <http://rdaregistry.info/Elements/i/> ;
        reg:status                <http://metadataregistry.org/uri/RegStatus/1001> ;
        reg:name                  "formerOwnerAgent"@en ;
        rdfs:label                "has former owner agent"@en ;
        skos:definition           "Relates an item to an agent who has former legal possession of an item."@en ;
        rdf:type                  rdf:Property ;
        rdfs:domain               <http://rdaregistry.info/Elements/c/C10003> ;
        rdfs:subPropertyOf        <http://rdaregistry.info/Elements/i/P40021> ;
        reg:hasSubproperty        <http://rdaregistry.info/Elements/i/P40007> ;
        reg:hasSubproperty        <http://rdaregistry.info/Elements/i/P40008> ;
        reg:lexicalAlias          <http://rdaregistry.info/Elements/i/formerOwnerAgent.en> ;
        reg:hasUnconstrained      <http://rdaregistry.info/Elements/u/P60401> ;
        rdakit:toolkitLabel       "former owner agent"@en ;
        rdakit:toolkitDefinition  "An agent who has former legal possession of an item."@en ;
        rdfs:label                "a pour ancien agent propriétaire"@fr ;
        skos:definition           "Met un item en relation avec un agent qui a auparavant possédé légalement un item."@fr ;
        rdakit:toolkitLabel       "ancien agent propriétaire"@fr ;
        rdakit:toolkitDefinition  "Agent qui a auparavant possédé légalement un item."@fr ;
        rdakit:toolkitLabel       "propietario anterior"@es ;
        rdakit:toolkitDefinition  "Una persona, familia o entidad corporativa que tuvo anteriormente la posesión legal de un ítem."@es ;
        rdakit:instructionNumber  "18.5" ;
        reg:hasSubproperty        <http://rdaregistry.info/Elements/i/object/P40019> ;
        reg:name                  "ngườiChủTrướcĐây"@vi ;
        rdfs:label                "có người chủ trước đây"@vi ;
        skos:definition           "Liên kết bản với tác nhân trước đây đã sở hữu theo pháp luật một bản."@vi ;
        rdakit:toolkitLabel       "người chủ trước đây"@vi ;
        rdakit:toolkitDefinition  "Tác nhân trước đây đã sở hữu theo pháp luật một bản."@vi ;
        reg:name                  "tidligereEjer"@da ;
        rdfs:label                "har tidligere ejer"@da ;
        reg:lexicalAlias          <http://rdaregistry.info/Elements/i/tidligereEjer.da> ;
        skos:definition           "Relaterer et eksemplar til en agent, der tidligere har været i lovlig besiddelse af et eksemplar."@da ;
        rdakit:toolkitLabel       "tidligere ejer"@da ;
        rdakit:toolkitDefinition  "Agent, der tidligere har været i lovlig besiddelse af et eksemplar."@da ;
        rdfs:label                "hat früheren Eigentümer"@de ;
        skos:definition           "Setzt ein Exemplar mit einem Akteur, der früher im rechtmäßigen Besitz eines Exemplars war, in Beziehung."@de ;
        rdakit:toolkitLabel       "Früherer Eigentümer"@de ;
        rdakit:toolkitDefinition  "Ein Akteur, der früher im rechtmäßigen Besitz eines Exemplars war."@de ;
        reg:name                  "προηγούμενοςΙδιοκτήτης"@el ;
        rdfs:label                "έχει προηγούμενο ιδιοκτήτη"@el ;
        reg:lexicalAlias          <http://rdaregistry.info/Elements/i/προηγούμενοςΙδιοκτήτης.el> ;
        skos:definition           "Συνδέει ένα αντίτυπο με έναν φορέα που είχε προηγούμενα τη νόμιμη κατοχή ενός αντιτύπου."@el ;
        rdakit:toolkitLabel       "προηγούμενος ιδιοκτήτης"@el ;
        rdakit:toolkitDefinition  "Ένας φορέας ο οποίος είχε προηγούμενα τη νόμιμη κατοχή ενός αντιτύπου."@el ;
        rdfs:label                "té com a propietari anterior"@ca ;
        skos:definition           "Relaciona un item amb un agent que anteriorment posseïa legalment un ítem."@ca ;
        rdakit:toolkitLabel       "propietari anterior"@ca ;
        rdakit:toolkitDefinition  "Agent que anteriorment posseïa legalment un ítem."@ca ;
        reg:name                  "aikaisempiOmistaja"@fi ;
        rdfs:label                "aikaisempi omistaja"@fi ;
        reg:lexicalAlias          <rdaa:aikaisempiOmistaja.fi> ;
        skos:definition           "Liittää kappaleen toimijaan, joka on aikaisemmin laillisesti omistanut kappaleen."@fi ;
        rdakit:toolkitLabel       "aikaisempi omistaja"@fi ;
        rdakit:toolkitDefinition  "Toimija, joka on aikaisemmin laillisesti omistanut kappaleen."@fi ;
        reg:name                  "ancienPropriétaire"@fr ;
        reg:lexicalAlias          <http://rdaregistry.info/Elements/i/ancienAgentPropriétaire.fr> ;
        rdakit:toolkitLabel       "tidligere eier"@no ;
        rdakit:toolkitDefinition  "En agent som tidligere var den rettmessige eieren av et eksemplar."@no ;
        rdakit:hasElementType     "2" ;
        reg:name                  "korábbiTulajdonos"@hu ;
        rdfs:label                "van korábbi tulajdonosa"@hu ;
        skos:definition           "Egy példányt hozzákapcsol egy ágenshez (személyhez, családhoz vagy testülethez), akinek/amelynek jogszerű tulajdonában volt. Korábban egy példány. "@hu ;
        rdakit:toolkitLabel       "korábbi tulajdonos"@hu ;
        rdakit:toolkitDefinition  "Egy ágens (személy, család vagy testület), akinek/amelynek korábban jogos tulajdonában volt egy példány."@hu ;
        skos:altLabel             "former owner"@en ;
        reg:hasSubproperty        <http://rdaregistry.info/Elements/i/P40108> ;
        reg:hasSubproperty        <http://rdaregistry.info/Elements/i/P40109> ;
        reg:hasSubproperty        <http://rdaregistry.info/Elements/i/P40124> ;
        reg:hasSubproperty        <http://rdaregistry.info/Elements/i/P40125> ;
        skos:altLabel             "ancien propriétaire"@fr .

<http://rdaregistry.info/Elements/i/P40118>
        rdfs:isDefinedBy          <http://rdaregistry.info/Elements/i/> ;
        reg:status                <http://metadataregistry.org/uri/RegStatus/1001> ;
        rdfs:label                "has former owner collective agent"@en ;
        reg:lexicalAlias          <http://rdaregistry.info/Elements/i/formerOwnerCollectiveAgent.en> ;
        skos:definition           "Relates an item to a collective agent who has former legal possession of an item."@en ;
        rdakit:toolkitLabel       "former owner collective agent"@en ;
        rdakit:toolkitDefinition  "A collective agent who has former legal possession of an item."@en ;
        rdf:type                  rdf:Property ;
        reg:name                  "formerOwnerCollectiveAgent" ;
        rdfs:domain               <http://rdaregistry.info/Elements/c/C10003> ;
        rdakit:hasElementType     "2" ;
        reg:hasSubproperty        <http://rdaregistry.info/Elements/i/datatype/P40118> ;
        reg:hasSubproperty        <http://rdaregistry.info/Elements/i/object/P40118> ;
        rdfs:subPropertyOf        <http://rdaregistry.info/Elements/i/P40120> ;
        rdfs:subPropertyOf        <http://rdaregistry.info/Elements/i/P40019> ;
        reg:hasSubproperty        <http://rdaregistry.info/Elements/i/P40124> ;
        reg:hasSubproperty        <http://rdaregistry.info/Elements/i/P40125> ;
        reg:hasSubproperty        <http://rdaregistry.info/Elements/i/P40134> ;
        reg:hasSubproperty        <http://rdaregistry.info/Elements/i/P40150> ;
        reg:hasUnconstrained      <http://rdaregistry.info/Elements/u/P60401> ;
        rdfs:label                "a pour ancien agent collectif propriétaire"@fr ;
        skos:definition           "Met un item en relation avec un agent collectif qui a auparavant possédé légalement un item."@fr ;
        rdakit:toolkitLabel       "ancien agent collectif propriétaire"@fr ;
        rdakit:toolkitDefinition  "Agent collectif qui a auparavant possédé légalement un item."@fr ;
        reg:lexicalAlias          <http://rdaregistry.info/Elements/i/ancienAgentCollectifPropriétaire.fr> .

<http://rdaregistry.info/Elements/i/P40134>
        rdfs:isDefinedBy          <http://rdaregistry.info/Elements/i/> ;
        reg:status                <http://metadataregistry.org/uri/RegStatus/1001> ;
        rdfs:label                "has former owner corporate body"@en ;
        reg:lexicalAlias          <http://rdaregistry.info/Elements/i/formerOwnerCorporateBody.en> ;
        skos:definition           "Relates an item to a corporate body who has former legal possession of an item."@en ;
        rdakit:toolkitLabel       "former owner corporate body"@en ;
        rdakit:toolkitDefinition  "A corporate body who has former legal possession of an item."@en ;
        rdf:type                  rdf:Property ;
        reg:name                  "formerOwnerCorporateBody" ;
        rdfs:domain               <http://rdaregistry.info/Elements/c/C10003> ;
        rdakit:hasElementType     "2" ;
        reg:hasSubproperty        <http://rdaregistry.info/Elements/i/datatype/P40134> ;
        reg:hasSubproperty        <http://rdaregistry.info/Elements/i/object/P40134> ;
        rdfs:subPropertyOf        <http://rdaregistry.info/Elements/i/P40136> ;
        rdfs:subPropertyOf        <http://rdaregistry.info/Elements/i/P40118> ;
        reg:hasSubproperty        <http://rdaregistry.info/Elements/i/P40140> ;
        reg:hasSubproperty        <http://rdaregistry.info/Elements/i/P40141> ;
        reg:hasUnconstrained      <http://rdaregistry.info/Elements/u/P60401> ;
        rdfs:label                "a pour ancienne collectivité propriétaire"@fr ;
        skos:definition           "Met un item en relation avec une collectivité qui a auparavant possédé légalement un item."@fr ;
        rdakit:toolkitLabel       "ancienne collectivité propriétaire"@fr ;
        rdakit:toolkitDefinition  "Collectivité qui a auparavant possédé légalement un item."@fr ;
        reg:lexicalAlias          <http://rdaregistry.info/Elements/i/ancienneCollectivitéPropriétaire.fr> .

<http://rdaregistry.info/Elements/i/P40150>
        rdfs:isDefinedBy          <http://rdaregistry.info/Elements/i/> ;
        reg:status                <http://metadataregistry.org/uri/RegStatus/1001> ;
        rdfs:label                "has former owner family"@en ;
        reg:lexicalAlias          <http://rdaregistry.info/Elements/i/formerOwnerFamily.en> ;
        skos:definition           "Relates an item to a family who has former legal possession of an item."@en ;
        rdakit:toolkitLabel       "former owner family"@en ;
        rdakit:toolkitDefinition  "A family who has former legal possession of an item."@en ;
        rdf:type                  rdf:Property ;
        reg:name                  "formerOwnerFamily" ;
        rdfs:domain               <http://rdaregistry.info/Elements/c/C10003> ;
        rdakit:hasElementType     "2" ;
        reg:hasSubproperty        <http://rdaregistry.info/Elements/i/datatype/P40150> ;
        reg:hasSubproperty        <http://rdaregistry.info/Elements/i/object/P40150> ;
        rdfs:subPropertyOf        <http://rdaregistry.info/Elements/i/P40152> ;
        rdfs:subPropertyOf        <http://rdaregistry.info/Elements/i/P40118> ;
        reg:hasSubproperty        <http://rdaregistry.info/Elements/i/P40156> ;
        reg:hasSubproperty        <http://rdaregistry.info/Elements/i/P40157> ;
        reg:hasUnconstrained      <http://rdaregistry.info/Elements/u/P60401> ;
        rdfs:label                "a pour ancienne famille propriétaire"@fr ;
        skos:definition           "Met un item en relation avec une famille qui a auparavant possédé légalement un item."@fr ;
        rdakit:toolkitLabel       "ancienne famille propriétaire"@fr ;
        rdakit:toolkitDefinition  "Famille qui a auparavant possédé légalement un item."@fr ;
        reg:lexicalAlias          <http://rdaregistry.info/Elements/i/ancienneFamillePropriétaire.fr> .

<http://rdaregistry.info/Elements/i/P40102>
        rdfs:isDefinedBy          <http://rdaregistry.info/Elements/i/> ;
        reg:status                <http://metadataregistry.org/uri/RegStatus/1001> ;
        rdfs:label                "has former owner person"@en ;
        reg:lexicalAlias          <http://rdaregistry.info/Elements/i/formerOwnerPerson.en> ;
        skos:definition           "Relates an item to a person who has former legal possession of an item."@en ;
        rdakit:toolkitLabel       "former owner person"@en ;
        rdakit:toolkitDefinition  "A person who has former legal possession of an item."@en ;
        rdf:type                  rdf:Property ;
        reg:name                  "formerOwnerPerson" ;
        rdfs:domain               <http://rdaregistry.info/Elements/c/C10003> ;
        rdakit:hasElementType     "2" ;
        reg:hasSubproperty        <http://rdaregistry.info/Elements/i/datatype/P40102> ;
        reg:hasSubproperty        <http://rdaregistry.info/Elements/i/object/P40102> ;
        rdfs:subPropertyOf        <http://rdaregistry.info/Elements/i/P40104> ;
        rdfs:subPropertyOf        <http://rdaregistry.info/Elements/i/P40019> ;
        reg:hasSubproperty        <http://rdaregistry.info/Elements/i/P40108> ;
        reg:hasSubproperty        <http://rdaregistry.info/Elements/i/P40109> ;
        reg:hasUnconstrained      <http://rdaregistry.info/Elements/u/P60401> ;
        rdfs:label                "a pour ancienne personne propriétaire"@fr ;
        skos:definition           "Met un item en relation avec une personne qui a auparavant possédé légalement un item."@fr ;
        rdakit:toolkitLabel       "ancienne personne propriétaire"@fr ;
        rdakit:toolkitDefinition  "Personne qui a auparavant possédé légalement un item."@fr ;
        reg:lexicalAlias          <http://rdaregistry.info/Elements/i/anciennePersonnePropriétaire.fr> .

<http://rdaregistry.info/Elements/i/P40052>
        rdfs:isDefinedBy    <http://rdaregistry.info/Elements/i/> ;
        reg:status          <http://metadataregistry.org/uri/RegStatus/1008> ;
        rdf:type            rdf:Property ;
        rdfs:subPropertyOf  <http://rdaregistry.info/Elements/i/P40046> ;
        reg:hasSubproperty  <http://rdaregistry.info/Elements/i/P40030> .

<http://rdaregistry.info/Elements/i/P40022>
        rdfs:isDefinedBy          <http://rdaregistry.info/Elements/i/> ;
        reg:status                <http://metadataregistry.org/uri/RegStatus/1001> ;
        reg:name                  "honoureeAgentOfItem"@en ;
        rdfs:label                "has honouree agent of item"@en ;
        skos:definition           "Relates an item to an agent who is honoured by an item."@en ;
        rdf:type                  rdf:Property ;
        rdfs:domain               <http://rdaregistry.info/Elements/c/C10003> ;
        rdfs:subPropertyOf        <http://rdaregistry.info/Elements/i/P40072> ;
        reg:lexicalAlias          <http://rdaregistry.info/Elements/i/honoureeAgentOfItem.en> ;
        reg:hasUnconstrained      <http://rdaregistry.info/Elements/u/P60406> ;
        skos:altLabel             "honoree of item"@en ;
        rdakit:toolkitLabel       "honouree agent of item"@en ;
        rdakit:toolkitDefinition  "An agent who is honoured by an item."@en ;
        rdfs:label                "a pour agent honoré d’un item"@fr ;
        skos:definition           "Met un item en relation avec un agent qui est honoré par un item."@fr ;
        rdakit:toolkitLabel       "agent honoré d’un item"@fr ;
        rdakit:toolkitDefinition  "Agent qui est honoré par un item."@fr ;
        rdakit:toolkitLabel       "homenajeado en el ítem"@es ;
        rdakit:toolkitDefinition  "Una persona, familia o entidad corporativa en cuyo honor se realiza un ítem, por ej., una persona a la cual se le brinda una copia."@es ;
        rdakit:instructionNumber  "18.5" ;
        reg:hasSubproperty        <http://rdaregistry.info/Elements/i/object/P40022> ;
        reg:name                  "ngườiKínhTrọngCủaBản"@vi ;
        rdfs:label                "có người kính trọng của bản"@vi ;
        skos:definition           "Liên kết bản với tác nhân được thể hiện kính trong bởi một bản."@vi ;
        rdakit:toolkitLabel       "người kính trọng (bản)"@vi ;
        rdakit:toolkitDefinition  "Tác nhân được thể hiện kính trong bởi một bản."@vi ;
        reg:name                  "festskriftmodtagerAfEksemplar"@da ;
        rdfs:label                "har festskriftmodtager(eksemplar)"@da ;
        reg:lexicalAlias          <http://rdaregistry.info/Elements/i/festskriftmodtagerAfEksemplar.da> ;
        skos:definition           "Relaterer et eksemplar til en agent, der hædres af et eksemplar."@da ;
        rdakit:toolkitLabel       "festskriftmodtager (eksemplar)"@da ;
        rdakit:toolkitDefinition  "Agent, der hædres af et eksemplar."@da ;
        rdfs:label                "hat Gefeierten (Exemplar)"@de ;
        skos:definition           "Setzt ein Exemplar mit einem Akteur, der durch ein Exemplar geehrt wird, in Beziehung."@de ;
        rdakit:toolkitLabel       "Gefeierter (Exemplar)"@de ;
        rdakit:toolkitDefinition  "Ein Akteur, der durch ein Exemplar geehrt wird."@de ;
        reg:name                  "τιμώμενοΠρόσωποΤουΑντιτύπου"@el ;
        rdfs:label                "έχει τιμώμενο πρόσωπο (αντίτυπο)"@el ;
        reg:lexicalAlias          <http://rdaregistry.info/Elements/i/τιμώμενοΠρόσωποΤουΑντιτύπου.el> ;
        skos:definition           "Συνδέει ένα αντίτυπο με έναν φορέα τιμώμενο σε ένα αντίτυπο."@el ;
        rdakit:toolkitLabel       "τιμώμενο πρόσωπο (αντίτυπο)"@el ;
        rdakit:toolkitDefinition  "Ένας φορέας τιμώμενος σε ένα αντίτυπο."@el ;
        rdfs:label                "té com a entitat honorada (ítem)"@ca ;
        skos:definition           "Relaciona un item amb un agent honorat en un ítem."@ca ;
        rdakit:toolkitLabel       "entitat honorada (ítem)"@ca ;
        rdakit:toolkitDefinition  "Agent honorat en un ítem."@ca ;
        reg:name                  "kappaleellaKunnioitettu"@fi ;
        rdfs:label                "kappaleella kunnioitettu"@fi ;
        reg:lexicalAlias          <rdaa:kappaleellaKunnioitettu.fi> ;
        skos:definition           "Liittää kappaleen toimijaan, jolle kappale on lahjoitettu kunnianosoituksena."@fi ;
        rdakit:toolkitLabel       "kappaleella kunnioitettu"@fi ;
        rdakit:toolkitDefinition  "Toimija, jolle kappale on lahjoitettu kunnianosoituksena."@fi ;
        reg:name                  "agentHonoréItem"@fr ;
        reg:lexicalAlias          <http://rdaregistry.info/Elements/i/agentHonoréDunItem.fr> ;
        rdakit:toolkitLabel       "beæret person (eksemplar)"@no ;
        rdakit:toolkitDefinition  "En agent som beæres av et eksemplar."@no ;
        rdakit:hasElementType     "2" ;
        reg:name                  "Példánydíjazottja"@hu ;
        rdfs:label                "van díjazottja (példány)"@hu ;
        skos:definition           "Egy példányt hozzákapcsol egy ágenshez (személyhez, családhoz vagy testülethez), akit/amelyet megtisztelnek egy példánnyal."@hu ;
        rdakit:toolkitLabel       "díjazott (példány)"@hu ;
        rdakit:toolkitDefinition  "Egy ágens (személy, család vagy testület), akit/amelyet kitűntettek egy példánnyal."@hu ;
        reg:hasSubproperty        <http://rdaregistry.info/Elements/i/datatype/P40022> ;
        skos:altLabel             "agent honoré (item)"@fr ;
        skos:altLabel             "honouree (item)"@en .

<http://rdaregistry.info/Elements/i/P40126>
        rdfs:isDefinedBy          <http://rdaregistry.info/Elements/i/> ;
        reg:status                <http://metadataregistry.org/uri/RegStatus/1001> ;
        rdfs:label                "has honouree collective agent of item"@en ;
        reg:lexicalAlias          <http://rdaregistry.info/Elements/i/honoureeCollectiveAgentOfItem.en> ;
        skos:definition           "Relates an item to a collective agent who is honoured by an item."@en ;
        rdakit:toolkitLabel       "honouree collective agent of item"@en ;
        rdakit:toolkitDefinition  "A collective agent who is honoured by an item."@en ;
        rdf:type                  rdf:Property ;
        reg:name                  "honoureeCollectiveAgentOfItem" ;
        rdfs:domain               <http://rdaregistry.info/Elements/c/C10003> ;
        rdakit:hasElementType     "2" ;
        reg:hasSubproperty        <http://rdaregistry.info/Elements/i/datatype/P40126> ;
        reg:hasSubproperty        <http://rdaregistry.info/Elements/i/object/P40126> ;
        rdfs:subPropertyOf        <http://rdaregistry.info/Elements/i/P40076> ;
        rdfs:subPropertyOf        <http://rdaregistry.info/Elements/i/P40022> ;
        reg:hasSubproperty        <http://rdaregistry.info/Elements/i/P40142> ;
        reg:hasSubproperty        <http://rdaregistry.info/Elements/i/P40158> ;
        reg:hasUnconstrained      <http://rdaregistry.info/Elements/u/P60406> ;
        rdfs:label                "a pour agent collectif honoré d’un item"@fr ;
        skos:definition           "Met un item en relation avec un agent collectif qui est honoré par un item."@fr ;
        rdakit:toolkitLabel       "agent collectif honoré d’un item"@fr ;
        rdakit:toolkitDefinition  "Agent collectif qui est honoré par un item."@fr ;
        reg:lexicalAlias          <http://rdaregistry.info/Elements/i/agentCollectifHonoréDunItem.fr> .

<http://rdaregistry.info/Elements/i/P40142>
        rdfs:isDefinedBy          <http://rdaregistry.info/Elements/i/> ;
        reg:status                <http://metadataregistry.org/uri/RegStatus/1001> ;
        rdfs:label                "has honouree corporate body of item"@en ;
        reg:lexicalAlias          <http://rdaregistry.info/Elements/i/honoureeCorporateBodyOfItem.en> ;
        skos:definition           "Relates an item to a corporate body who is honoured by an item."@en ;
        rdakit:toolkitLabel       "honouree corporate body of item"@en ;
        rdakit:toolkitDefinition  "A corporate body who is honoured by an item."@en ;
        rdf:type                  rdf:Property ;
        reg:name                  "honoureeCorporateBodyOfItem" ;
        rdfs:domain               <http://rdaregistry.info/Elements/c/C10003> ;
        rdakit:hasElementType     "2" ;
        reg:hasSubproperty        <http://rdaregistry.info/Elements/i/datatype/P40142> ;
        reg:hasSubproperty        <http://rdaregistry.info/Elements/i/object/P40142> ;
        rdfs:subPropertyOf        <http://rdaregistry.info/Elements/i/P40075> ;
        rdfs:subPropertyOf        <http://rdaregistry.info/Elements/i/P40126> ;
        reg:hasUnconstrained      <http://rdaregistry.info/Elements/u/P60406> ;
        rdfs:label                "a pour collectivité honorée d’un item"@fr ;
        skos:definition           "Met un item en relation avec une collectivité qui est honorée par un item."@fr ;
        rdakit:toolkitLabel       "collectivité honorée d’un item"@fr ;
        rdakit:toolkitDefinition  "Collectivité qui est honorée par un item."@fr ;
        reg:lexicalAlias          <http://rdaregistry.info/Elements/i/collectivitéHonoréeDunItem.fr> .

<http://rdaregistry.info/Elements/i/P40158>
        rdfs:isDefinedBy          <http://rdaregistry.info/Elements/i/> ;
        reg:status                <http://metadataregistry.org/uri/RegStatus/1001> ;
        rdfs:label                "has honouree family of item"@en ;
        reg:lexicalAlias          <http://rdaregistry.info/Elements/i/honoureeFamilyOfItem.en> ;
        skos:definition           "Relates an item to a family who is honoured by an item."@en ;
        rdakit:toolkitLabel       "honouree family of item"@en ;
        rdakit:toolkitDefinition  "A family who is honoured by an item."@en ;
        rdf:type                  rdf:Property ;
        reg:name                  "honoureeFamilyOfItem" ;
        rdfs:domain               <http://rdaregistry.info/Elements/c/C10003> ;
        rdakit:hasElementType     "2" ;
        reg:hasSubproperty        <http://rdaregistry.info/Elements/i/datatype/P40158> ;
        reg:hasSubproperty        <http://rdaregistry.info/Elements/i/object/P40158> ;
        rdfs:subPropertyOf        <http://rdaregistry.info/Elements/i/P40074> ;
        rdfs:subPropertyOf        <http://rdaregistry.info/Elements/i/P40126> ;
        reg:hasUnconstrained      <http://rdaregistry.info/Elements/u/P60406> ;
        rdfs:label                "a pour famille honorée d’un item"@fr ;
        skos:definition           "Met un item en relation avec une famille qui est honorée par un item."@fr ;
        rdakit:toolkitLabel       "famille honorée d’un item"@fr ;
        rdakit:toolkitDefinition  "Famille qui est honorée par un item."@fr ;
        reg:lexicalAlias          <http://rdaregistry.info/Elements/i/familleHonoréeDunItem.fr> .

<http://rdaregistry.info/Elements/i/P40110>
        rdfs:isDefinedBy          <http://rdaregistry.info/Elements/i/> ;
        reg:status                <http://metadataregistry.org/uri/RegStatus/1001> ;
        rdfs:label                "has honouree person of item"@en ;
        reg:lexicalAlias          <http://rdaregistry.info/Elements/i/honoureePersonOfItem.en> ;
        skos:definition           "Relates an item to a person who is honoured by an item."@en ;
        rdakit:toolkitLabel       "honouree person of item"@en ;
        rdakit:toolkitDefinition  "A person who is honoured by an item."@en ;
        rdf:type                  rdf:Property ;
        reg:name                  "honoureePersonOfItem" ;
        rdfs:domain               <http://rdaregistry.info/Elements/c/C10003> ;
        rdakit:hasElementType     "2" ;
        reg:hasSubproperty        <http://rdaregistry.info/Elements/i/datatype/P40110> ;
        reg:hasSubproperty        <http://rdaregistry.info/Elements/i/object/P40110> ;
        rdfs:subPropertyOf        <http://rdaregistry.info/Elements/i/P40073> ;
        rdfs:subPropertyOf        <http://rdaregistry.info/Elements/i/P40022> ;
        reg:hasUnconstrained      <http://rdaregistry.info/Elements/u/P60406> ;
        rdfs:label                "a pour personne honorée d’un item"@fr ;
        skos:definition           "Met un item en relation avec une personne qui est honorée par un item."@fr ;
        rdakit:toolkitLabel       "personne honorée d’un item"@fr ;
        rdakit:toolkitDefinition  "Personne qui est honorée par un item."@fr ;
        reg:lexicalAlias          <http://rdaregistry.info/Elements/i/personneHonoréeDunItem.fr> .

<http://rdaregistry.info/Elements/i/P40001>
        rdfs:isDefinedBy          <http://rdaregistry.info/Elements/i/> ;
        reg:status                <http://metadataregistry.org/uri/RegStatus/1001> ;
        reg:name                  "identifierForItem"@en ;
        rdfs:label                "has identifier for item"@en ;
        skos:definition           "Relates an item to an appellation of item that consists of a code, number, or other string, usually independent of natural language and social naming conventions, used to identify an item."@en ;
        rdf:type                  rdf:Property ;
        rdfs:domain               <http://rdaregistry.info/Elements/c/C10003> ;
        reg:lexicalAlias          <http://rdaregistry.info/Elements/i/identifierForItem.en> ;
        reg:hasUnconstrained      <http://rdaregistry.info/Elements/u/P60052> ;
        rdakit:instructionNumber  "2.20" ;
        rdakit:toolkitLabel       "identifier for item"@en ;
        rdakit:toolkitDefinition  "An appellation of item that consists of a code, number, or other string, usually independent of natural language and social naming conventions, used to identify an item."@en ;
        rdfs:label                "a pour identifiant d’item"@fr ;
        skos:definition           "Met un item en relation avec une appellation d’item qui consiste en un code, un nombre ou une autre chaîne, généralement indépendante du langage naturel et des conventions sociales de dénomination, utilisée pour identifier un item."@fr ;
        rdakit:toolkitLabel       "identifiant d’item"@fr ;
        rdakit:toolkitDefinition  "Appellation d’item qui consiste en un code, un nombre ou une autre chaîne, généralement indépendante du langage naturel et des conventions sociales de dénomination, utilisée pour identifier un item."@fr ;
        rdakit:toolkitLabel       "identificador del ítem"@es ;
        rdakit:toolkitDefinition  "Una cadena de caracteres asociada con un ítem que sirve para diferenciar ese ítem de otros ítems"@es ;
        reg:hasSubproperty        <http://rdaregistry.info/Elements/i/object/P40001> ;
        rdfs:label                "har identifikator för exemplaret"@sv ;
        rdakit:toolkitLabel       "identifikator för exemplaret"@sv ;
        reg:name                  "chỉSốNhậnDạngCủaBản"@vi ;
        rdfs:label                "có chỉ số nhận dạng của bản"@vi ;
        skos:definition           "Liên kết bản với chuỗi ký tự liên quan với bản phục vụ để phân biệt một bản với các bản khác."@vi ;
        rdakit:toolkitLabel       "chỉ số nhận dạng của bản"@vi ;
        rdakit:toolkitDefinition  "Chuỗi ký tự liên quan với bản phục vụ để phân biệt một bản với các bản khác."@vi ;
        reg:name                  "identifikatorForEksemplaret"@da ;
        rdfs:label                "har identifikator for eksemplaret"@da ;
        reg:lexicalAlias          <http://rdaregistry.info/Elements/i/identifikatorForEksemplaret.da> ;
        skos:definition           "Relaterer et eksemplar til en tegnrække, der er knyttet til et eksemplar, der tjener til at skelne dette eksemplar fra andre eksemplarer."@da ;
        rdakit:toolkitLabel       "identifikator for eksemplaret"@da ;
        rdakit:toolkitDefinition  "Tegnrække, der er knyttet til et eksemplar, der tjener til at skelne dette eksemplar fra andre eksemplarer."@da ;
        rdfs:label                "hat Identifikator für ein Exemplar"@de ;
        skos:definition           "Setzt ein Exemplar mit einer Zeichenfolge, die mit einem Exemplar in Verbindung steht und dazu dient, dieses Exemplar von anderen Exemplaren zu unterscheiden, in Beziehung."@de ;
        rdakit:toolkitLabel       "Identifikator für ein Exemplar"@de ;
        rdakit:toolkitDefinition  "Eine Zeichenfolge, die mit einem Exemplar in Verbindung steht und dazu dient, dieses Exemplar von anderen Exemplaren zu unterscheiden."@de ;
        reg:name                  "αναγνωριστικόΓιαΑντίτυπο"@el ;
        rdfs:label                "έχει αναγνωριστικό για αντίτυπο"@el ;
        reg:lexicalAlias          <http://rdaregistry.info/Elements/i/αναγνωριστικόΓιαΑντίτυπο.el> ;
        skos:definition           "Συνδέει ένα αντίτυπο με έναν αλφαριθμητικό χαρακτήρα συνδεδεμένο με ένα αντίτυπο με σκοπό τη διαφοροποίηση ενός αντιτύπου από άλλα αντίτυπα."@el ;
        rdakit:toolkitLabel       "αναγνωριστικό για αντίτυπο"@el ;
        rdakit:toolkitDefinition  "Ένας αλφαριθμητικός χαρακτήρας συνδεδεμένος με ένα αντίτυπο με σκοπό τη διαφοροποίηση ενός αντιτύπου από άλλα αντίτυπα."@el ;
        rdfs:label                "té com a identificador d’ítem"@ca ;
        skos:definition           "Relaciona un item amb una cadena de caràcters associada amb un ítem que serveix per diferenciar un ítem d’altres ítems."@ca ;
        rdakit:toolkitLabel       "identificador d’ítem"@ca ;
        rdakit:toolkitDefinition  "Cadena de caràcters associada amb un ítem que serveix per diferenciar un ítem d’altres ítems."@ca ;
        reg:name                  "kappaleenTunniste"@fi ;
        rdfs:label                "kappaleen tunniste"@fi ;
        reg:lexicalAlias          <rdaa:kappaleenTunniste.fi> ;
        skos:definition           "Viittauksen kohde on merkkijono, joka liittyy kappaleeseen ja erottaa sen muista kappaleista."@fi ;
        rdakit:toolkitLabel       "kappaleen tunniste"@fi ;
        rdakit:toolkitDefinition  "Merkkijono, joka liittyy kappaleeseen ja erottaa sen muista kappaleista."@fi ;
        reg:name                  "identifiantDitem"@fr ;
        reg:lexicalAlias          <http://rdaregistry.info/Elements/i/identifiantDitem.fr> ;
        rdakit:toolkitLabel       "identifikator for eksemplar"@no ;
        rdakit:toolkitDefinition  "En tegnstreng som forbindes med et eksemplar og hvis formål er å skille et eksemplar fra andre eksemplarer."@no ;
        rdfs:subPropertyOf        <http://rdaregistry.info/Elements/i/P40081> ;
        rdakit:hasElementType     "3" ;
        reg:name                  "Példányazonosítója"@hu ;
        rdfs:label                "van példányazonosítója"@hu ;
        skos:definition           "Egy példányt hozzákapcsol egy példányhoz kötődő karakterlánchoz, amely egy példány más példányoktól való megkülönböztetésére szolgál."@hu ;
        rdakit:toolkitLabel       "példányazonosító"@hu ;
        rdakit:toolkitDefinition  "Egy példányhoz kötődő karakterlánc, amely arra szolgál, hogy egy példányt más példányoktól megkülönböztessen. "@hu ;
        reg:hasSubproperty        <http://rdaregistry.info/Elements/i/datatype/P40001> ;
        rdfs:subPropertyOf        <http://rdaregistry.info/Elements/x/P00018> .

<http://rdaregistry.info/Elements/i/P40012>
        rdfs:isDefinedBy          <http://rdaregistry.info/Elements/i/> ;
        reg:status                <http://metadataregistry.org/uri/RegStatus/1001> ;
        reg:name                  "illuminatorAgent"@en ;
        rdfs:label                "has illuminator agent"@en ;
        skos:definition           "Relates an item to an agent who decorates a specific item using precious metals or colour, often with elaborate designs and motifs."@en ;
        rdf:type                  rdf:Property ;
        rdfs:domain               <http://rdaregistry.info/Elements/c/C10003> ;
        rdfs:subPropertyOf        <http://rdaregistry.info/Elements/i/P40093> ;
        reg:lexicalAlias          <http://rdaregistry.info/Elements/i/illuminatorAgent.en> ;
        reg:hasUnconstrained      <http://rdaregistry.info/Elements/u/P60421> ;
        rdakit:toolkitLabel       "illuminator agent"@en ;
        rdakit:toolkitDefinition  "An agent who decorates a specific item using precious metals or colour, often with elaborate designs and motifs."@en ;
        rdfs:label                "a pour agent enlumineur"@fr ;
        skos:definition           "Met un item en relation avec un agent qui orne un item spécifique en utilisant des métaux précieux ou de la couleur, souvent avec des dessins et des motifs élaborés."@fr ;
        rdakit:toolkitLabel       "agent enlumineur"@fr ;
        rdakit:toolkitDefinition  "Agent qui orne un item spécifique en utilisant des métaux précieux ou de la couleur, souvent avec des dessins et des motifs élaborés."@fr ;
        rdakit:toolkitLabel       "iluminador"@es ;
        rdakit:toolkitDefinition  "Una persona que proporciona la decoración de un ítem específico utilizando metales preciosos, o color, a menudo con diseños y motivos elaborados."@es ;
        rdakit:instructionNumber  "18.5" ;
        reg:hasSubproperty        <http://rdaregistry.info/Elements/i/object/P40012> ;
        reg:name                  "ngườiTôMàu"@vi ;
        rdfs:label                "có người tô màu"@vi ;
        skos:definition           "Liên kết bản với cá nhân trang trí cho bản cụ thể sử dụng kim loại quý hoặc màu, thường thiết kế và kiểu dáng tỷ mỷ."@vi ;
        rdakit:toolkitLabel       "người tô màu"@vi ;
        rdakit:toolkitDefinition  "Cá nhân trang trí cho bản cụ thể sử dụng kim loại quý hoặc màu, thường thiết kế và kiểu dáng tỷ mỷ."@vi ;
        reg:name                  "illuminator"@da ;
        rdfs:label                "har illuminator"@da ;
        reg:lexicalAlias          <http://rdaregistry.info/Elements/i/illuminator.da> ;
        skos:definition           "Relaterer et eksemplar til en person, der har tilført et særligt eksemplar en udsmykning vha. ædelmetal eller farve, ofte med udsøgte designs og motiver."@da ;
        rdakit:toolkitLabel       "illuminator"@da ;
        rdakit:toolkitDefinition  "Person, der har tilført et særligt eksemplar en udsmykning vha. ædelmetal eller farve, ofte med udsøgte designs og motiver."@da ;
        rdfs:label                "hat Illuminator"@de ;
        skos:definition           "Setzt ein Exemplar mit einer Person, die ein bestimmtes Exemplar durch Edelmetalle oder Farben (aus-)gestaltet, häufig mit kunstvollen Mustern und Motiven, in Beziehung."@de ;
        rdakit:toolkitLabel       "Illuminator"@de ;
        rdakit:toolkitDefinition  "Eine Person, die ein bestimmtes Exemplar durch Edelmetalle oder Farben (aus-)gestaltet, häufig mit kunstvollen Mustern und Motiven."@de ;
        reg:name                  "φωτιστής"@el ;
        rdfs:label                "έχει φωτιστή"@el ;
        reg:lexicalAlias          <http://rdaregistry.info/Elements/i/φωτιστής.el> ;
        skos:definition           "Συνδέει ένα αντίτυπο με ένα φυσικό πρόσωπο που διακοσμεί ένα συγκεκριμένο αντίτυπο χρησιμοποιώντας πολύτιμα μέταλλα ή χρώματα, συχνά με περίτεχνα σχέδια και μοτίβα."@el ;
        rdakit:toolkitLabel       "φωτιστής"@el ;
        rdakit:toolkitDefinition  "Ένα φυσικό πρόσωπο που διακοσμεί ένα συγκεκριμένο αντίτυπο χρησιμοποιώντας πολύτιμα μέταλλα ή χρώματα, συχνά με περίτεχνα σχέδια και μοτίβα."@el ;
        rdfs:label                "té com a il·luminador"@ca ;
        skos:definition           "Relaciona un item amb una persona que decora un ítem concret amb metalls preciosos o amb color, sovint amb dissenys i motius elaborats."@ca ;
        rdakit:toolkitLabel       "il·luminador"@ca ;
        rdakit:toolkitDefinition  "Persona que decora un ítem concret amb metalls preciosos o amb color, sovint amb dissenys i motius elaborats."@ca ;
        reg:name                  "illuminoinninTekija"@fi ;
        rdfs:label                "illuminoinnin tekijä"@fi ;
        reg:lexicalAlias          <rdaa:illuminoinninTekija.fi> ;
        skos:definition           "Liittää kappaleen henkilöön, joka on koristellut kappaleen käyttäen jalometalleja tai värejä, usein yksityiskohtaisilla kuvioilla tai aiheilla."@fi ;
        rdakit:toolkitLabel       "illuminoinnin tekijä"@fi ;
        rdakit:toolkitDefinition  "Henkilö, joka on koristellut kappaleen käyttäen jalometalleja tai värejä, usein yksityiskohtaisilla kuvioilla tai aiheilla."@fi ;
        reg:name                  "enlumineur"@fr ;
        reg:lexicalAlias          <http://rdaregistry.info/Elements/i/agentEnlumineur.fr> ;
        rdakit:toolkitLabel       "illuminator"@no ;
        rdakit:toolkitDefinition  "En person som dekorerer et bestemt eksemplar med edle metaller eller farger, gjerne med intrikate former og motiver."@no ;
        rdakit:hasElementType     "2" ;
        reg:name                  "illuminátor"@hu ;
        rdfs:label                "van illuminátora"@hu ;
        skos:definition           "Egy példányt hozzákapcsol egy személyhez, aki dekorációval lát el egy sajátos példányt nemesfémek vagy színek használatával, gyakran kimunkált dizájnnal és motívumokkal. "@hu ;
        rdakit:toolkitLabel       "illuminátor"@hu ;
        rdakit:toolkitDefinition  "Egy személy, aki egy adott példányt díszítéssel lát el nemesfémek vagy színek használatával, gyakran gondosan megmunkált formamintákkal és motívumokkal."@hu ;
        reg:hasSubproperty        <http://rdaregistry.info/Elements/i/datatype/P40012> ;
        skos:altLabel             "illuminator"@en ;
        skos:altLabel             "enlumineur"@fr .

<http://rdaregistry.info/Elements/i/P40116>
        rdfs:isDefinedBy          <http://rdaregistry.info/Elements/i/> ;
        reg:status                <http://metadataregistry.org/uri/RegStatus/1001> ;
        rdfs:label                "has illuminator collective agent"@en ;
        reg:lexicalAlias          <http://rdaregistry.info/Elements/i/illuminatorCollectiveAgent.en> ;
        skos:definition           "Relates an item to a collective agent who decorates a specific item using precious metals or colour, often with elaborate designs and motifs."@en ;
        rdakit:toolkitLabel       "illuminator collective agent"@en ;
        rdakit:toolkitDefinition  "A collective agent who decorates a specific item using precious metals or colour, often with elaborate designs and motifs."@en ;
        rdf:type                  rdf:Property ;
        reg:name                  "illuminatorCollectiveAgent" ;
        rdfs:domain               <http://rdaregistry.info/Elements/c/C10003> ;
        rdakit:hasElementType     "2" ;
        reg:hasSubproperty        <http://rdaregistry.info/Elements/i/datatype/P40116> ;
        reg:hasSubproperty        <http://rdaregistry.info/Elements/i/object/P40116> ;
        rdfs:subPropertyOf        <http://rdaregistry.info/Elements/i/P40128> ;
        rdfs:subPropertyOf        <http://rdaregistry.info/Elements/i/P40012> ;
        reg:hasSubproperty        <http://rdaregistry.info/Elements/i/P40132> ;
        reg:hasSubproperty        <http://rdaregistry.info/Elements/i/P40148> ;
        reg:hasUnconstrained      <http://rdaregistry.info/Elements/u/P60421> ;
        rdfs:label                "a pour agent collectif enlumineur"@fr ;
        skos:definition           "Met un item en relation avec un agent collectif qui orne un item spécifique en utilisant des métaux précieux ou de la couleur, souvent avec des dessins et des motifs élaborés."@fr ;
        rdakit:toolkitLabel       "agent collectif enlumineur"@fr ;
        rdakit:toolkitDefinition  "Agent collectif qui orne un item spécifique en utilisant des métaux précieux ou de la couleur, souvent avec des dessins et des motifs élaborés."@fr ;
        reg:lexicalAlias          <http://rdaregistry.info/Elements/i/agentCollectifEnlumineur.fr> .

<http://rdaregistry.info/Elements/i/P40132>
        rdfs:isDefinedBy          <http://rdaregistry.info/Elements/i/> ;
        reg:status                <http://metadataregistry.org/uri/RegStatus/1001> ;
        rdfs:label                "has illuminator corporate body"@en ;
        reg:lexicalAlias          <http://rdaregistry.info/Elements/i/illuminatorCorporateBody.en> ;
        skos:definition           "Relates an item to a corporate body who decorates a specific item using precious metals or colour, often with elaborate designs and motifs."@en ;
        rdakit:toolkitLabel       "illuminator corporate body"@en ;
        rdakit:toolkitDefinition  "A corporate body who decorates a specific item using precious metals or colour, often with elaborate designs and motifs."@en ;
        rdf:type                  rdf:Property ;
        reg:name                  "illuminatorCorporateBody" ;
        rdfs:domain               <http://rdaregistry.info/Elements/c/C10003> ;
        rdakit:hasElementType     "2" ;
        reg:hasSubproperty        <http://rdaregistry.info/Elements/i/datatype/P40132> ;
        reg:hasSubproperty        <http://rdaregistry.info/Elements/i/object/P40132> ;
        rdfs:subPropertyOf        <http://rdaregistry.info/Elements/i/P40144> ;
        rdfs:subPropertyOf        <http://rdaregistry.info/Elements/i/P40116> ;
        reg:hasUnconstrained      <http://rdaregistry.info/Elements/u/P60421> ;
        rdfs:label                "a pour collectivité enlumineuse"@fr ;
        skos:definition           "Met un item en relation avec une collectivité qui orne un item spécifique en utilisant des métaux précieux ou de la couleur, souvent avec des dessins et des motifs élaborés."@fr ;
        rdakit:toolkitLabel       "collectivité enlumineuse"@fr ;
        rdakit:toolkitDefinition  "Collectivité qui orne un item spécifique en utilisant des métaux précieux ou de la couleur, souvent avec des dessins et des motifs élaborés."@fr ;
        reg:lexicalAlias          <http://rdaregistry.info/Elements/i/collectivitéEnlumineuse.fr> .

<http://rdaregistry.info/Elements/i/P40148>
        rdfs:isDefinedBy          <http://rdaregistry.info/Elements/i/> ;
        reg:status                <http://metadataregistry.org/uri/RegStatus/1001> ;
        rdfs:label                "has illuminator family"@en ;
        reg:lexicalAlias          <http://rdaregistry.info/Elements/i/illuminatorFamily.en> ;
        skos:definition           "Relates an item to a family who decorates a specific item using precious metals or colour, often with elaborate designs and motifs."@en ;
        rdakit:toolkitLabel       "illuminator family"@en ;
        rdakit:toolkitDefinition  "A family who decorates a specific item using precious metals or colour, often with elaborate designs and motifs."@en ;
        rdf:type                  rdf:Property ;
        reg:name                  "illuminatorFamily" ;
        rdfs:domain               <http://rdaregistry.info/Elements/c/C10003> ;
        rdakit:hasElementType     "2" ;
        reg:hasSubproperty        <http://rdaregistry.info/Elements/i/datatype/P40148> ;
        reg:hasSubproperty        <http://rdaregistry.info/Elements/i/object/P40148> ;
        rdfs:subPropertyOf        <http://rdaregistry.info/Elements/i/P40160> ;
        rdfs:subPropertyOf        <http://rdaregistry.info/Elements/i/P40116> ;
        reg:hasUnconstrained      <http://rdaregistry.info/Elements/u/P60421> ;
        rdfs:label                "a pour famille enlumineuse"@fr ;
        skos:definition           "Met un item en relation avec une famille qui orne un item spécifique en utilisant des métaux précieux ou de la couleur, souvent avec des dessins et des motifs élaborés."@fr ;
        rdakit:toolkitLabel       "famille enlumineuse"@fr ;
        rdakit:toolkitDefinition  "Famille qui orne un item spécifique en utilisant des métaux précieux ou de la couleur, souvent avec des dessins et des motifs élaborés."@fr ;
        reg:lexicalAlias          <http://rdaregistry.info/Elements/i/familleEnlumineuse.fr> .

<http://rdaregistry.info/Elements/i/P40100>
        rdfs:isDefinedBy          <http://rdaregistry.info/Elements/i/> ;
        reg:status                <http://metadataregistry.org/uri/RegStatus/1001> ;
        rdfs:label                "has illuminator person"@en ;
        reg:lexicalAlias          <http://rdaregistry.info/Elements/i/illuminatorPerson.en> ;
        skos:definition           "Relates an item to a person who decorates a specific item using precious metals or colour, often with elaborate designs and motifs."@en ;
        rdakit:toolkitLabel       "illuminator person"@en ;
        rdakit:toolkitDefinition  "A person who decorates a specific item using precious metals or colour, often with elaborate designs and motifs."@en ;
        rdf:type                  rdf:Property ;
        reg:name                  "illuminatorPerson" ;
        rdfs:domain               <http://rdaregistry.info/Elements/c/C10003> ;
        rdakit:hasElementType     "2" ;
        reg:hasSubproperty        <http://rdaregistry.info/Elements/i/datatype/P40100> ;
        reg:hasSubproperty        <http://rdaregistry.info/Elements/i/object/P40100> ;
        rdfs:subPropertyOf        <http://rdaregistry.info/Elements/i/P40112> ;
        rdfs:subPropertyOf        <http://rdaregistry.info/Elements/i/P40012> ;
        reg:hasUnconstrained      <http://rdaregistry.info/Elements/u/P60421> ;
        rdfs:label                "a pour personne enlumineuse"@fr ;
        skos:definition           "Met un item en relation avec une personne qui orne un item spécifique en utilisant des métaux précieux ou de la couleur, souvent avec des dessins et des motifs élaborés."@fr ;
        rdakit:toolkitLabel       "personne enlumineuse"@fr ;
        rdakit:toolkitDefinition  "Personne qui orne un item spécifique en utilisant des métaux précieux ou de la couleur, souvent avec des dessins et des motifs élaborés."@fr ;
        reg:lexicalAlias          <http://rdaregistry.info/Elements/i/personneEnlumineuse.fr> .

<http://rdaregistry.info/Elements/i/P40050>
        rdfs:isDefinedBy          <http://rdaregistry.info/Elements/i/> ;
        reg:status                <http://metadataregistry.org/uri/RegStatus/1001> ;
        reg:name                  "immediateSourceOfAcquisitionOfItem"@en ;
        rdfs:label                "has immediate source of acquisition of item"@en ;
        skos:definition           "Relates an item to the circumstances under which an item is directly acquired, including a method, source, and date of acquisition."@en ;
        rdf:type                  rdf:Property ;
        rdfs:domain               <http://rdaregistry.info/Elements/c/C10003> ;
        reg:lexicalAlias          <http://rdaregistry.info/Elements/i/immediateSourceOfAcquisitionOfItem.en> ;
        reg:hasUnconstrained      <http://rdaregistry.info/Elements/u/P60583> ;
        rdakit:instructionNumber  "2.19" ;
        rdakit:toolkitLabel       "immediate source of acquisition of item"@en ;
        rdakit:toolkitDefinition  "The circumstances under which an item is directly acquired, including a method, source, and date of acquisition."@en ;
        rdfs:label                "a pour source immédiate d’acquisition d’un item"@fr ;
        skos:definition           "Met un item en relation avec des circonstances dans lesquelles un item a été directement acquis, notamment une méthode, une source et une date d’acquisition."@fr ;
        rdakit:toolkitLabel       "source immédiate d’acquisition d’un item"@fr ;
        rdakit:toolkitDefinition  "Circonstances dans lesquelles un item a été directement acquis, notamment une méthode, une source et une date d’acquisition."@fr ;
        rdakit:toolkitLabel       "fuente inmediata de acquisición del ítem"@es ;
        rdakit:toolkitDefinition  "La fuente de la cual la agencia adquirió directamente un ítem y las circunstancias bajo las cuales se recibió."@es ;
        reg:hasSubproperty        <http://rdaregistry.info/Elements/i/object/P40050> ;
        rdfs:label                "har senaste förvärvskälla"@sv ;
        rdakit:toolkitLabel       "senaste förvärvskälla"@sv ;
        reg:name                  "nguồnBổSungTrựcTiếpCủaBản"@vi ;
        rdfs:label                "có nguồn bổ sung trực tiếp của bản"@vi ;
        skos:definition           "Liên kết bản với nguồn mà từ đó cơ quan bổ sung trực tiếp bản và điều kiện quy định để nhận được nó."@vi ;
        rdakit:toolkitLabel       "nguồn bổ sung trực tiếp của bản"@vi ;
        rdakit:toolkitDefinition  "Nguồn mà từ đó cơ quan bổ sung trực tiếp bản và điều kiện quy định để nhận được nó."@vi ;
        reg:name                  "direkteAnskaffelseskildeForEksemplar"@da ;
        rdfs:label                "har direkte anskaffelseskilde for eksemplar"@da ;
        reg:lexicalAlias          <http://rdaregistry.info/Elements/i/direkteAnskaffelseskildeForEksemplar.da> ;
        skos:definition           "Relaterer et eksemplar til en kilde, hvorfra institutionen har anskaffet et eksemplar, samt de omstændigheder under hvilke det blev modtaget."@da ;
        rdakit:toolkitLabel       "direkte anskaffelseskilde for eksemplar"@da ;
        rdakit:toolkitDefinition  "Kilde, hvorfra institutionen har anskaffet et eksemplar, samt de omstændigheder under hvilke det blev modtaget."@da ;
        rdfs:label                "hat Bezugsquelle des Exemplars"@de ;
        skos:definition           "Setzt ein Exemplar mit einer Quelle, aus der eine Agentur ein Exemplar direkt erworben hat, und die Umstände, unter denen sie es erhalten hat, in Beziehung."@de ;
        rdakit:toolkitLabel       "Bezugsquelle des Exemplars"@de ;
        rdakit:toolkitDefinition  "Die Quelle, aus der eine Agentur ein Exemplar direkt erworben hat, und die Umstände, unter denen sie es erhalten hat."@de ;
        reg:name                  "άμεσηΠηγήΤηςΠρόσκτησηςΤουΑντιτύπου"@el ;
        rdfs:label                "έχει άμεση πηγή της πρόσκτησης του αντιτύπου"@el ;
        reg:lexicalAlias          <http://rdaregistry.info/Elements/i/άμεσηΠηγήΤηςΠρόσκτησηςΤουΑντιτύπου.el> ;
        skos:definition           "Συνδέει ένα αντίτυπο με μια πηγή από την οποία ένας φορέας απέκτησε άμεσα ένα αντίτυπο και τις συνθήκες υπό τις οποίες το παρέλαβε."@el ;
        rdakit:toolkitLabel       "άμεση πηγή της πρόσκτησης του αντιτύπου"@el ;
        rdakit:toolkitDefinition  "Μια πηγή από την οποία ένας φορέας απέκτησε άμεσα ένα αντίτυπο και οι συνθήκες υπό τις οποίες το παρέλαβε."@el ;
        rdfs:label                "té com a font immediata d’adquisició"@ca ;
        skos:definition           "Relaciona un item amb una font a partir de la qual una agència va adquirir directament un ítem i les circumstàncies en què es va rebre."@ca ;
        rdakit:toolkitLabel       "font immediata d’adquisició"@ca ;
        rdakit:toolkitDefinition  "Font a partir de la qual una agència va adquirir directament un ítem i les circumstàncies en què es va rebre."@ca ;
        reg:name                  "kappaleenHankintalahde"@fi ;
        rdfs:label                "kappaleen hankintalähde"@fi ;
        reg:lexicalAlias          <rdaa:kappaleenHankintalahde.fi> ;
        skos:definition           "Liittää kappaleen kappaleen hankintaan liittyvään lähteeseen ja muihin hankintaan liittyviin yksityiskohtiin."@fi ;
        rdakit:toolkitLabel       "kappaleen hankintalähde"@fi ;
        rdakit:toolkitDefinition  "Kappaleen hankintaan liittyvä lähde ja muita hankintaan liittyviä yksityiskohtia."@fi ;
        reg:name                  "sourceImmédiateDacquisitionDunItem"@fr ;
        reg:lexicalAlias          <http://rdaregistry.info/Elements/i/sourceImmédiateDacquisitionDunItem.fr> ;
        rdakit:toolkitLabel       "direkte kilde for anskaffelse av eksemplar"@no ;
        rdakit:toolkitDefinition  "En kilde som en institusjon har anskaffet et eksemplar direkte fra, og omstendighetene eksemplaret ble anskaffet under."@no ;
        rdakit:hasElementType     "6" ;
        reg:name                  "PéldányközvetlenBeszerzésiforrás"@hu ;
        rdfs:label                "van közvetlen példánybeszerzési forrása"@hu ;
        skos:definition           "Egy példányt hozzákapcsol egy forráshoz, amelytől egy ügynökség közvetlenül beszerzett egy példányt és azok a körülmények, amelyek között azt megkapták. "@hu ;
        rdakit:toolkitLabel       "példány közvetlen beszerzési forrása"@hu ;
        rdakit:toolkitDefinition  "Egy forrás, amelyből egy ügynökség közvetlenül szerzett be egy példányt, és a körülmények, amelyek közepette azt megkapták."@hu ;
        reg:hasSubproperty        <http://rdaregistry.info/Elements/i/datatype/P40050> .

<http://rdaregistry.info/Elements/i/P40014>
        rdfs:isDefinedBy          <http://rdaregistry.info/Elements/i/> ;
        reg:status                <http://metadataregistry.org/uri/RegStatus/1001> ;
        reg:name                  "inscriber"@en ;
        rdfs:label                "has inscriber"@en ;
        skos:definition           "Relates an item to a person who writes a statement of dedication or gift on an item."@en ;
        rdf:type                  rdf:Property ;
        rdfs:domain               <http://rdaregistry.info/Elements/c/C10003> ;
        rdfs:subPropertyOf        <http://rdaregistry.info/Elements/i/P40112> ;
        reg:lexicalAlias          <http://rdaregistry.info/Elements/i/inscriber.en> ;
        reg:hasUnconstrained      <http://rdaregistry.info/Elements/u/P60460> ;
        rdakit:toolkitLabel       "inscriber"@en ;
        rdakit:toolkitDefinition  "A person who writes a statement of dedication or gift on an item."@en ;
        rdfs:label                "a pour dédicateur d’un item"@fr ;
        skos:definition           "Met un item en relation avec une personne qui écrit une dédicace ou une mention de don sur un item."@fr ;
        rdakit:toolkitLabel       "dédicateur d’un item"@fr ;
        rdakit:toolkitDefinition  "Personne qui écrit une dédicace ou une mention de don sur un item."@fr ;
        rdakit:toolkitLabel       "autor de dedicatoria"@es ;
        rdakit:toolkitDefinition  "Una persona que ha escrito una mención de dedicatoria o donación en un ítem."@es ;
        rdakit:instructionNumber  "18.5" ;
        reg:hasSubproperty        <http://rdaregistry.info/Elements/i/object/P40014> ;
        reg:name                  "ngườiGhi"@vi ;
        rdfs:label                "có người khắc"@vi ;
        skos:definition           "Liên kết bản với cá nhân người viết thông tin đề tặng hoặc quà biếu trên bản."@vi ;
        rdakit:toolkitLabel       "người ghi"@vi ;
        rdakit:toolkitDefinition  "Cá nhân người viết thông tin đề tặng hoặc quà biếu trên bản."@vi ;
        reg:name                  "dedikationsskriver"@da ;
        rdfs:label                "har dedikationsskriver"@da ;
        reg:lexicalAlias          <http://rdaregistry.info/Elements/i/dedikationsskriver.da> ;
        skos:definition           "Relaterer et eksemplar til en person, der har skrevet en tilegnelses- eller gavekommentar på et eksemplar."@da ;
        rdakit:toolkitLabel       "dedikationsskriver"@da ;
        rdakit:toolkitDefinition  "Person, der har skrevet en tilegnelses- eller gavekommentar på et eksemplar."@da ;
        rdfs:label                "hat beschriftende Person"@de ;
        skos:definition           "Setzt ein Exemplar mit einer Person, die eine Widmung oder einen Schenkungsvermerk in ein Exemplar geschrieben hat, in Beziehung."@de ;
        rdakit:toolkitLabel       "Beschriftende Person"@de ;
        rdakit:toolkitDefinition  "Eine Person, die eine Widmung oder einen Schenkungsvermerk in ein Exemplar geschrieben hat."@de ;
        reg:name                  "χαράκτης"@el ;
        rdfs:label                "έχει χαράκτη"@el ;
        reg:lexicalAlias          <http://rdaregistry.info/Elements/i/χαράκτης.el> ;
        skos:definition           "Συνδέει ένα αντίτυπο με ένα φυσικό πρόσωπο το οποίο έχει γράψει μια αφιέρωση ή δήλωση δωρεάς σε ένα αντίτυπο."@el ;
        rdakit:toolkitLabel       "χαράκτης"@el ;
        rdakit:toolkitDefinition  "Ένα φυσικό πρόσωπο το οποίο έχει γράψει μια αφιέρωση ή δήλωση δωρεάς σε ένα αντίτυπο."@el ;
        rdfs:label                "té com a inscriptor"@ca ;
        skos:definition           "Relaciona un item amb una persona que ha escrit una menció de dedicatòria o de regal en un ítem."@ca ;
        rdakit:toolkitLabel       "inscriptor"@ca ;
        rdakit:toolkitDefinition  "Persona que ha escrit una menció de dedicatòria o de regal en un ítem."@ca ;
        reg:name                  "omistuskirjoituksenKirjoittaja"@fi ;
        rdfs:label                "omistuskirjoituksen kirjoittaja"@fi ;
        reg:lexicalAlias          <rdaa:omistuskirjoituksenKirjoittaja.fi> ;
        skos:definition           "Liittää kappaleen henkilöön, joka on kirjoittanut kappaleeseen omistuskirjoituksen tai merkinnän lahjoituksesta."@fi ;
        rdakit:toolkitLabel       "omistuskirjoituksen kirjoittaja"@fi ;
        rdakit:toolkitDefinition  "Henkilö, joka on kirjoittanut kappaleeseen omistuskirjoituksen tai merkinnän lahjoituksesta."@fi ;
        reg:name                  "dédicateurItem"@fr ;
        reg:lexicalAlias          <http://rdaregistry.info/Elements/i/dédicateurDunItem.fr> ;
        rdakit:toolkitLabel       "person som tilegner"@no ;
        rdakit:toolkitDefinition  "En person som har skrevet en tilegnelse i et eksemplar."@no ;
        rdakit:hasElementType     "2" ;
        reg:name                  "beíró"@hu ;
        rdfs:label                "van beírója"@hu ;
        skos:definition           "Egy példányt hozzákapcsol egy személyhez, aki egy példányról ajánlási vagy ajándékozási nyilatkozatot írt."@hu ;
        rdakit:toolkitLabel       "beíró"@hu ;
        rdakit:toolkitDefinition  "Egy személy, aki ajánlási vagy adományozási nyilatkozatot írt egy példányra."@hu ;
        reg:hasSubproperty        <http://rdaregistry.info/Elements/i/datatype/P40014> .

<http://rdaregistry.info/Elements/i/P40063>
        rdfs:isDefinedBy          <http://rdaregistry.info/Elements/i/> ;
        reg:status                <http://metadataregistry.org/uri/RegStatus/1001> ;
        rdf:type                  rdf:Property ;
        reg:name                  "itemAnalysedIn"@en ;
        rdfs:label                "is item analysed in"@en ;
        reg:lexicalAlias          <http://rdaregistry.info/Elements/i/itemAnalysedIn.en> ;
        skos:definition           "Relates an item to a work that describes the structure and composition of an item."@en ;
        rdfs:domain               <http://rdaregistry.info/Elements/c/C10003> ;
        reg:hasUnconstrained      <http://rdaregistry.info/Elements/u/P60219> ;
        rdakit:toolkitLabel       "item analysed in"@en ;
        rdakit:toolkitDefinition  "A work that describes the structure and composition of an item."@en ;
        rdfs:label                "est un item analysé dans"@fr ;
        skos:definition           "Met un item en relation avec une œuvre qui décrit la structure et la composition d’un item."@fr ;
        rdakit:toolkitLabel       "item analysé dans"@fr ;
        rdakit:toolkitDefinition  "Œuvre qui décrit la structure et la composition d’un item."@fr ;
        rdakit:toolkitLabel       "analizada en (ítem)"@es ;
        rdakit:toolkitDefinition  "Una obra que examina el ítem fuente para identificar sus componentes y sus relaciones."@es ;
        rdfs:subPropertyOf        <http://rdaregistry.info/Elements/i/P40062> ;
        rdakit:instructionNumber  "23.5" ;
        reg:hasSubproperty        <http://rdaregistry.info/Elements/i/object/P40063> ;
        reg:name                  "đượcPhânTíchTrongBản"@vi ;
        rdfs:label                "được phân tích trong (bản)"@vi ;
        skos:definition           "Liên kết bản với tác phẩm kiểm tra bản nguồn để nhận dạng các thành phần của nó và quan hệ của chúng."@vi ;
        rdakit:toolkitLabel       "được phân tích trong (bản)"@vi ;
        rdakit:toolkitDefinition  "Tác phẩm kiểm tra bản nguồn để nhận dạng các thành phần của nó và quan hệ của chúng."@vi ;
        reg:name                  "analyseretIEksemplar"@da ;
        rdfs:label                "er analyseret i (eksemplar)"@da ;
        reg:lexicalAlias          <http://rdaregistry.info/Elements/i/analyseretIEksemplar.da> ;
        skos:definition           "Relaterer et eksemplar til et værk, der undersøger et oprindeligt eksemplar for at identificere dets dele og deres relationer."@da ;
        rdakit:toolkitLabel       "analyseret i (eksemplar)"@da ;
        rdakit:toolkitDefinition  "Værk, der undersøger et oprindeligt eksemplar for at identificere dets dele og deres relationer."@da ;
        rdfs:label                "ist analysiert in (Exemplar)"@de ;
        skos:definition           "Setzt ein Exemplar mit einem Werk, das ein ursprüngliches Exemplar untersucht, um seine Bestandteile und deren Beziehungen zu identifizieren, in Beziehung."@de ;
        rdakit:toolkitLabel       "Analysiert in (Exemplar)"@de ;
        rdakit:toolkitDefinition  "Ein Werk, das ein ursprüngliches Exemplar untersucht, um seine Bestandteile und deren Beziehungen zu identifizieren."@de ;
        reg:name                  "αναλύεταιΣτοΑντίτυπο"@el ;
        rdfs:label                "αναλύεται στο (αντίτυπο)"@el ;
        reg:lexicalAlias          <http://rdaregistry.info/Elements/i/αναλύεταιΣτοΑντίτυπο.el> ;
        skos:definition           "Συνδέει ένα αντίτυπο με ένα έργο που εξετάζει ένα αντίτυπο-πηγή για την ταύτιση των συστατικών του και των σχέσεων τους."@el ;
        rdakit:toolkitLabel       "αναλύεται στο (αντίτυπο)"@el ;
        rdakit:toolkitDefinition  "Ένα έργο που εξετάζει ένα αντίτυπο-πηγή για την ταύτιση των συστατικών του και των σχέσεων τους."@el ;
        rdfs:label                "és analitzat en (ítem)"@ca ;
        skos:definition           "Relaciona un item amb una obra que examina un ítem font per identificar els seus components i les seves relacions."@ca ;
        rdakit:toolkitLabel       "analitzat en (ítem)"@ca ;
        rdakit:toolkitDefinition  "Obra que examina un ítem font per identificar els seus components i les seves relacions."@ca ;
        reg:name                  "kappaleenAnalyysi"@fi ;
        rdfs:label                "kappaleen analyysi"@fi ;
        reg:lexicalAlias          <rdaa:kappaleenAnalyysi.fi> ;
        skos:definition           "Liittää kappaleen teokseen, joka tutkii lähteenä olevan kappaleen osia ja niiden välisiä suhteita analyyttisesti."@fi ;
        rdakit:toolkitLabel       "kappaleen analyysi"@fi ;
        rdakit:toolkitDefinition  "Teos, joka tutkii lähteenä olevan kappaleen osia ja niiden välisiä suhteita analyyttisesti."@fi ;
        reg:name                  "analyséDansItem"@fr ;
        reg:lexicalAlias          <http://rdaregistry.info/Elements/i/itemAnalyséDans.fr> ;
        rdakit:toolkitLabel       "analysert i (eksemplar)"@no ;
        rdakit:toolkitDefinition  "Et verk som utforsker et kildeeksemplar for å identifisere kildeeksemplarets elementer og forhold mellom elementene."@no ;
        rdakit:hasElementType     "2" ;
        skos:altLabel             "analysed in (item)"@en ;
        reg:name                  "Példánybanelemezve"@hu ;
        rdfs:label                "elemezve (példány)"@hu ;
        skos:definition           "Egy példányt hozzákapcsol egy olyan műhöz, amely egy forráspéldányt vizsgál, hogy azonosítsa annak alkotóelemeit és azok viszonyait. "@hu ;
        rdakit:toolkitLabel       "elemezve (példány)"@hu ;
        rdakit:toolkitDefinition  "Egy mű, amely egy forráspéldányt vizsgál, hogy azonosítsa annak alkotóelemeit és azok viszonyait."@hu ;
        skos:altLabel             "analysé dans (item)"@fr .

<http://rdaregistry.info/Elements/i/P40064>
        rdfs:isDefinedBy          <http://rdaregistry.info/Elements/i/> ;
        reg:status                <http://metadataregistry.org/uri/RegStatus/1001> ;
        rdf:type                  rdf:Property ;
        reg:name                  "itemCommentaryIn"@en ;
        rdfs:label                "is item commentary in"@en ;
        reg:lexicalAlias          <http://rdaregistry.info/Elements/i/itemCommentaryIn.en> ;
        skos:definition           "Relates an item to a work that contains a set of explanatory or critical notes on an item."@en ;
        rdfs:domain               <http://rdaregistry.info/Elements/c/C10003> ;
        reg:hasUnconstrained      <http://rdaregistry.info/Elements/u/P60213> ;
        rdakit:toolkitLabel       "item commentary in"@en ;
        rdakit:toolkitDefinition  "A work that contains a set of explanatory or critical notes on an item."@en ;
        rdfs:label                "est un item commenté dans"@fr ;
        skos:definition           "Met un item en relation avec une œuvre qui contient un ensemble de notes explicatives ou critiques sur un item."@fr ;
        rdakit:toolkitLabel       "item commenté dans"@fr ;
        rdakit:toolkitDefinition  "Œuvre qui contient un ensemble de notes explicatives ou critiques sur un item."@fr ;
        rdakit:toolkitLabel       "comentario en (ítem)"@es ;
        rdakit:toolkitDefinition  "Una obra que contiene un conjunto de notas explicativas o críticas sobre el ítem descrito."@es ;
        rdfs:subPropertyOf        <http://rdaregistry.info/Elements/i/P40062> ;
        rdakit:instructionNumber  "23.5" ;
        reg:hasSubproperty        <http://rdaregistry.info/Elements/i/object/P40064> ;
        reg:name                  "bìnhLuậnTrongBản"@vi ;
        rdfs:label                "là bình luận trong (bản)"@vi ;
        skos:definition           "Liên kết bản với tác phẩm có chứa chuỗi các ghi chú giải thích hoặc phê bình về bản được mô tả."@vi ;
        rdakit:toolkitLabel       "bình luận trong (bản)"@vi ;
        rdakit:toolkitDefinition  "Tác phẩm có chứa chuỗi các ghi chú giải thích hoặc phê bình về bản được mô tả."@vi ;
        reg:name                  "kommentarIEksemplar"@da ;
        rdfs:label                "er kommentar i (eksemplar)"@da ;
        reg:lexicalAlias          <http://rdaregistry.info/Elements/i/kommentarIEksemplar.da> ;
        skos:definition           "Relaterer et eksemplar til et værk, der indeholder et sæt af forklarende eller kritiske noter om et beskrevet eksemplar."@da ;
        rdakit:toolkitLabel       "kommentar i eksemplar"@da ;
        rdakit:toolkitDefinition  "Værk, der indeholder et sæt af forklarende eller kritiske noter om et beskrevet eksemplar."@da ;
        rdfs:label                "ist Kommentar in (Exemplar)"@de ;
        skos:definition           "Setzt ein Exemplar mit einem Werk, das eine Reihe von erläuternden oder kritischen Anmerkungen zum beschriebenen Exemplar enthält, in Beziehung."@de ;
        rdakit:toolkitLabel       "Kommentar in (Exemplar)"@de ;
        rdakit:toolkitDefinition  "Ein Werk, das eine Reihe von erläuternden oder kritischen Anmerkungen zum beschriebenen Exemplar enthält."@de ;
        reg:name                  "σχόλιαΣτοΑντίτυπο"@el ;
        rdfs:label                "είναι σχόλια στο (αντίτυπο)"@el ;
        reg:lexicalAlias          <http://rdaregistry.info/Elements/i/σχόλιαΣτοΑντίτυπο.el> ;
        skos:definition           "Συνδέει ένα αντίτυπο με ένα έργο που περιέχει ένα σύνολο επεξηγηματικών ή κριτικών σημειώσεων σε ένα περιγραφόμενο αντίτυπο."@el ;
        rdakit:toolkitLabel       "σχόλια στο (αντίτυπο)"@el ;
        rdakit:toolkitDefinition  "Ένα έργο που περιέχει ένα σύνολο επεξηγηματικών ή κριτκών σημειώσεων σε ένα περιγραφόμενο αντίτυπο."@el ;
        rdfs:label                "és comentari en (ítem)"@ca ;
        skos:definition           "Relaciona un item amb una obra que inclou un conjunt de notes explicatives o crítiques sobre un ítem descrit."@ca ;
        rdakit:toolkitLabel       "comentari en (ítem)"@ca ;
        rdakit:toolkitDefinition  "Obra que inclou un conjunt de notes explicatives o crítiques sobre un ítem descrit."@ca ;
        reg:name                  "kappaleenKommentaari"@fi ;
        rdfs:label                "kappaleen kommentaari"@fi ;
        reg:lexicalAlias          <rdaa:kappaleenKommentaari.fi> ;
        skos:definition           "Liittää kappaleen teokseen, joka sisältää selittäviä tai kriittisiä huomautuksia kuvailun kohteena olevasta kappalesta."@fi ;
        rdakit:toolkitLabel       "kappaleen kommentaari"@fi ;
        rdakit:toolkitDefinition  "Teos, joka sisältää selittäviä tai kriittisiä huomautuksia kuvailun kohteena olevasta kappaleesta."@fi ;
        reg:name                  "commentaireDansItem"@fr ;
        reg:lexicalAlias          <http://rdaregistry.info/Elements/i/itemCommentéDans.fr> ;
        rdakit:toolkitLabel       "kommentar i (eksemplar)"@no ;
        rdakit:toolkitDefinition  "Et verk som inneholder et sett med forklarende eller kritiske noter til et eksemplar som beskrives."@no ;
        rdakit:hasElementType     "2" ;
        skos:altLabel             "commentary in (item)"@en ;
        reg:name                  "kommentárPéldányban"@hu ;
        rdfs:label                "kommentálva (példány)"@hu ;
        skos:definition           "Egy példányt hozzákapcsol egy olyan műhöz, amely  magyarázó vagy kritikai megjegyzések halmazát tartalmazza egy leírt példányról."@hu ;
        rdakit:toolkitLabel       "kommentálva (példány)"@hu ;
        rdakit:toolkitDefinition  "Egy mű, amely egy leírt példányról szóló magyarázati vagy kritikai megjegyzéshalmazt tartalmaz."@hu ;
        skos:altLabel             "commentaire dans (item)"@fr .

<http://rdaregistry.info/Elements/i/P40065>
        rdfs:isDefinedBy          <http://rdaregistry.info/Elements/i/> ;
        reg:status                <http://metadataregistry.org/uri/RegStatus/1001> ;
        rdf:type                  rdf:Property ;
        reg:name                  "itemCritiquedIn"@en ;
        rdfs:label                "is item critiqued in"@en ;
        reg:lexicalAlias          <http://rdaregistry.info/Elements/i/itemCritiquedIn.en> ;
        skos:definition           "Relates an item to a work that contains a critical evaluation of an item."@en ;
        rdfs:domain               <http://rdaregistry.info/Elements/c/C10003> ;
        reg:hasUnconstrained      <http://rdaregistry.info/Elements/u/P60212> ;
        rdakit:toolkitLabel       "item critiqued in"@en ;
        rdakit:toolkitDefinition  "A work that contains a critical evaluation of an item."@en ;
        rdfs:label                "est un item critiqué dans"@fr ;
        skos:definition           "Met un item en relation avec une œuvre qui contient une évaluation critique d’un item."@fr ;
        rdakit:toolkitLabel       "item critiqué dans"@fr ;
        rdakit:toolkitDefinition  "Œuvre qui contient une évaluation critique d’un item."@fr ;
        rdakit:toolkitLabel       "criticada en (ítem)"@es ;
        rdakit:toolkitDefinition  "Una obra que contiene una evaluación crítica del ítem descrito."@es ;
        rdfs:subPropertyOf        <http://rdaregistry.info/Elements/i/P40062> ;
        rdakit:instructionNumber  "23.5" ;
        reg:hasSubproperty        <http://rdaregistry.info/Elements/i/object/P40065> ;
        reg:name                  "đượcPhêBìnhTrongBản"@vi ;
        rdfs:label                "được phê bình trong (bản)"@vi ;
        skos:definition           "Liên kết bản với tác phẩm có chứa đánh giá phê bình về bản được mô tả."@vi ;
        rdakit:toolkitLabel       "được phê bình trong (bản)"@vi ;
        rdakit:toolkitDefinition  "Tác phẩm có chứa đánh giá phê bình về bản được mô tả."@vi ;
        reg:name                  "kritiseretIEksemplar"@da ;
        rdfs:label                "er kritiseret i (eksemplar)"@da ;
        reg:lexicalAlias          <http://rdaregistry.info/Elements/i/kritiseretIEksemplar.da> ;
        skos:definition           "Relaterer et eksemplar til et værk, der indeholder kritisk evaluering af et beskrevet eksemplar."@da ;
        rdakit:toolkitLabel       "kritiseret i (eksemplar)"@da ;
        rdakit:toolkitDefinition  "Værk, der indeholder en kritisk evaluering af et beskrevet eksemplar."@da ;
        rdfs:label                "ist Kritik in (Exemplar)"@de ;
        skos:definition           "Setzt ein Exemplar mit einem Werk, das eine kritische Untersuchung eines beschriebenen Exemplars enthält, in Beziehung."@de ;
        rdakit:toolkitLabel       "Kritik in (Exemplar)"@de ;
        rdakit:toolkitDefinition  "Ein Werk, das eine kritische Untersuchung eines beschriebenen Exemplars enthält."@de ;
        reg:name                  "κρίνεταιΣτοΑντίτυπο"@el ;
        rdfs:label                "κρίνεται στο (αντίτυπο)"@el ;
        reg:lexicalAlias          <http://rdaregistry.info/Elements/i/κρίνεταιΣτοΑντίτυπο.el> ;
        skos:definition           "Συνδέει ένα αντίτυπο με ένα έργο που περιέχει μια κριτική αξιολόγηση ενός περιγραφόμενου αντιτύπου."@el ;
        rdakit:toolkitLabel       "κρίνεται στο (αντίτυπο)"@el ;
        rdakit:toolkitDefinition  "Ένα έργο που περιέχει μια κριτική αξιολόγηση ενός περιγραφόμενου αντιτύπου."@el ;
        rdfs:label                "és criticat en (ítem)"@ca ;
        skos:definition           "Relaciona un item amb una obra que inclou una avaluació crítica d’un ítem descrit."@ca ;
        rdakit:toolkitLabel       "criticat en (ítem)"@ca ;
        rdakit:toolkitDefinition  "Obra que inclou una avaluació crítica d’un ítem descrit."@ca ;
        reg:name                  "kappaleenKritiikki"@fi ;
        rdfs:label                "kappaleen kritiikki"@fi ;
        reg:lexicalAlias          <rdaa:kappaleenKritiikki.fi> ;
        skos:definition           "Liittää kappaleen teokseen, joka sisältää kriittisen arvioinnin kuvailun kohteena olevasta kappalesta."@fi ;
        rdakit:toolkitLabel       "kappaleen kritiikki"@fi ;
        rdakit:toolkitDefinition  "Teos, joka sisältää kriittisen arvioinnin kuvailun kohteena olevasta kappaleesta."@fi ;
        reg:name                  "critiquéDansItem"@fr ;
        reg:lexicalAlias          <http://rdaregistry.info/Elements/i/itemCritiquéDans.fr> ;
        rdakit:toolkitLabel       "kritikk i (eksemplar)"@no ;
        rdakit:toolkitDefinition  "Et verk som inneholder en kritisk evaluering av et eksemplar som beskrives."@no ;
        rdakit:hasElementType     "2" ;
        skos:altLabel             "critiqued in (item)"@en ;
        reg:name                  "Példánybanbírálva"@hu ;
        rdfs:label                "bírálva (példány)"@hu ;
        skos:definition           "Egy példányt hozzákapcsol egy olyan műhöz, amely egy leírt példány kritikai értékelését tartalmazza."@hu ;
        rdakit:toolkitLabel       "bírálva (példány)"@hu ;
        rdakit:toolkitDefinition  "Egy mű, amely egy leírt példány kritikai értékelését tartalmazza."@hu ;
        skos:altLabel             "critiqué dans (item)"@fr .

<http://rdaregistry.info/Elements/i/P40062>
        rdfs:isDefinedBy          <http://rdaregistry.info/Elements/i/> ;
        reg:status                <http://metadataregistry.org/uri/RegStatus/1001> ;
        rdf:type                  rdf:Property ;
        reg:name                  "itemDescribedIn"@en ;
        rdfs:label                "is item described in"@en ;
        reg:lexicalAlias          <http://rdaregistry.info/Elements/i/itemDescribedIn.en> ;
        skos:definition           "Relates an item to a work that describes an item."@en ;
        rdfs:domain               <http://rdaregistry.info/Elements/c/C10003> ;
        reg:hasUnconstrained      <http://rdaregistry.info/Elements/u/P60215> ;
        rdakit:toolkitLabel       "item described in"@en ;
        rdakit:toolkitDefinition  "A work that describes an item."@en ;
        rdfs:label                "est un item décrit dans"@fr ;
        skos:definition           "Met un item en relation avec une œuvre qui décrit un item."@fr ;
        rdakit:toolkitLabel       "item décrit dans"@fr ;
        rdakit:toolkitDefinition  "Œuvre qui décrit un item."@fr ;
        rdakit:toolkitLabel       "descrita en (ítem)"@es ;
        rdakit:toolkitDefinition  "Una obra que describe un ítem descrito."@es ;
        rdfs:subPropertyOf        <http://rdaregistry.info/Elements/i/P40061> ;
        reg:hasSubproperty        <http://rdaregistry.info/Elements/i/P40063> ;
        reg:hasSubproperty        <http://rdaregistry.info/Elements/i/P40064> ;
        reg:hasSubproperty        <http://rdaregistry.info/Elements/i/P40065> ;
        reg:hasSubproperty        <http://rdaregistry.info/Elements/i/P40066> ;
        reg:hasSubproperty        <http://rdaregistry.info/Elements/i/P40067> ;
        rdakit:instructionNumber  "23.5" ;
        reg:hasSubproperty        <http://rdaregistry.info/Elements/i/object/P40062> ;
        reg:name                  "đượcMôTảTrongBản"@vi ;
        rdfs:label                "được mô tả trong (bản)"@vi ;
        skos:definition           "Liên kết bản với tác phẩm mô tả bản được mô tả."@vi ;
        rdakit:toolkitLabel       "được mô tả trong (bản)"@vi ;
        rdakit:toolkitDefinition  "Tác phẩm mô tả bản được mô tả."@vi ;
        reg:name                  "beskrevetIEksemplar"@da ;
        rdfs:label                "er beskrevet i (eksemplar)"@da ;
        reg:lexicalAlias          <http://rdaregistry.info/Elements/i/beskrevetIEksemplar.da> ;
        skos:definition           "Relaterer et eksemplar til et værk, der beskriver et beskrevet eksemplar."@da ;
        rdakit:toolkitLabel       "beskrevet i (eksemplar)"@da ;
        rdakit:toolkitDefinition  "Værk, der beskriver et beskrevet eksemplar."@da ;
        rdfs:label                "ist beschrieben in (Exemplar)"@de ;
        skos:definition           "Setzt ein Exemplar mit einem Werk, das ein beschriebenes Exemplar beschreibt, in Beziehung."@de ;
        rdakit:toolkitLabel       "Beschrieben in (Exemplar)"@de ;
        rdakit:toolkitDefinition  "Ein Werk, das ein beschriebenes Exemplar beschreibt."@de ;
        reg:name                  "περιγράφεταιΣτοΑντίτυπο"@el ;
        rdfs:label                "περιγράφεται στο (αντίτυπο)"@el ;
        reg:lexicalAlias          <http://rdaregistry.info/Elements/i/περιγράφεταιΣτοΑντίτυπο.el> ;
        skos:definition           "Συνδέει ένα αντίτυπο με ένα έργο που περιγράφει ένα περιγραφόμενο αντίτυπο."@el ;
        rdakit:toolkitLabel       "περιγράφεται στο (αντίτυπο)"@el ;
        rdakit:toolkitDefinition  "Ένα έργο που περιγράφει ένα περιγραφόμενο αντίτυπο."@el ;
        rdfs:label                "és descrit en (ítem)"@ca ;
        skos:definition           "Relaciona un item amb una obra que descriu un ítem descrit."@ca ;
        rdakit:toolkitLabel       "descrit en (ítem)"@ca ;
        rdakit:toolkitDefinition  "Obra que descriu un ítem descrit."@ca ;
        reg:name                  "kappaleenKuvaus"@fi ;
        rdfs:label                "kappaleen kuvaus"@fi ;
        reg:lexicalAlias          <rdaa:kappaleenKuvaus.fi> ;
        skos:definition           "Liittää kappaleen teokseen, joka kuvaa kuvattua kappaletta."@fi ;
        rdakit:toolkitLabel       "kappaleen kuvaus"@fi ;
        rdakit:toolkitDefinition  "Teos, joka kuvaa kuvattua kappaletta."@fi ;
        reg:name                  "décritDansItem"@fr ;
        reg:lexicalAlias          <http://rdaregistry.info/Elements/i/itemDécritDans.fr> ;
        rdakit:toolkitLabel       "beskrives i (eksemplar)"@no ;
        rdakit:toolkitDefinition  "Et verk som beskriver et eksemplar som beskrives."@no ;
        rdakit:hasElementType     "2" ;
        skos:altLabel             "described in (item)"@en ;
        reg:name                  "Példánybanleírva"@hu ;
        rdfs:label                "leírva (példány)"@hu ;
        skos:definition           "Egy példányt hozzákapcsol egy olyan műhöz, amely egy leírt példányt ír le."@hu ;
        rdakit:toolkitLabel       "leírva (példány)"@hu ;
        rdakit:toolkitDefinition  "Egy mű, amely egy leírt példányt ír le."@hu ;
        skos:altLabel             "décrit dans (item)"@fr .

<http://rdaregistry.info/Elements/i/P40066>
        rdfs:isDefinedBy          <http://rdaregistry.info/Elements/i/> ;
        reg:status                <http://metadataregistry.org/uri/RegStatus/1001> ;
        rdf:type                  rdf:Property ;
        reg:name                  "itemEvaluatedIn"@en ;
        rdfs:label                "is item evaluated in"@en ;
        reg:lexicalAlias          <http://rdaregistry.info/Elements/i/itemEvaluatedIn.en> ;
        skos:definition           "Relates an item to a work that examines or judges an item."@en ;
        rdfs:domain               <http://rdaregistry.info/Elements/c/C10003> ;
        reg:hasUnconstrained      <http://rdaregistry.info/Elements/u/P60218> ;
        rdakit:toolkitLabel       "item evaluated in"@en ;
        rdakit:toolkitDefinition  "A work that examines or judges an item."@en ;
        rdfs:label                "est un item évalué dans"@fr ;
        skos:definition           "Met un item en relation avec une œuvre qui examine ou juge un item."@fr ;
        rdakit:toolkitLabel       "item évalué dans"@fr ;
        rdakit:toolkitDefinition  "Œuvre qui examine ou juge un item."@fr ;
        rdakit:toolkitLabel       "evaluada en (ítem)"@es ;
        rdakit:toolkitDefinition  "Una obra que examina o juzga el ítem descrito."@es ;
        rdfs:subPropertyOf        <http://rdaregistry.info/Elements/i/P40062> ;
        rdakit:instructionNumber  "23.5" ;
        reg:hasSubproperty        <http://rdaregistry.info/Elements/i/object/P40066> ;
        reg:name                  "đượcĐánhGiáTrongBản"@vi ;
        rdfs:label                "được đánh giá trong (bản)"@vi ;
        skos:definition           "Liên kết bản với tác phẩm kiểm tra hoặc đánh giá bản đang được mô tả."@vi ;
        rdakit:toolkitLabel       "được đánh giá trong (bản)"@vi ;
        rdakit:toolkitDefinition  "Tác phẩm kiểm tra hoặc đánh giá bản đang được mô tả."@vi ;
        reg:name                  "evalueretIEksempalr"@da ;
        rdfs:label                "er evalueret i (eksemplar)"@da ;
        reg:lexicalAlias          <http://rdaregistry.info/Elements/i/evalueretIEksempalr.da> ;
        skos:definition           "Relaterer et eksemplar til et værk, der undersøger eller bedømmer et beskrevet eksemplar."@da ;
        rdakit:toolkitLabel       "evalueret i (eksemplar)"@da ;
        rdakit:toolkitDefinition  "Værk, der undersøger eller bedømmer et beskrevet eksemplar."@da ;
        rdfs:label                "ist evaluiert in (Exemplar)"@de ;
        skos:definition           "Setzt ein Exemplar mit einem Werk, das ein beschriebenes Exemplar untersucht oder beurteilt, in Beziehung."@de ;
        rdakit:toolkitLabel       "Evaluiert in (Exemplar)"@de ;
        rdakit:toolkitDefinition  "Ein Werk, das ein beschriebenes Exemplar untersucht oder beurteilt."@de ;
        reg:name                  "αξιολογείταιΣτοΑντίτυπο"@el ;
        rdfs:label                "αξιολογείται στο (αντίτυπο)"@el ;
        reg:lexicalAlias          <http://rdaregistry.info/Elements/i/αξιολογείταιΣτοΑντίτυπο.el> ;
        skos:definition           "Συνδέει ένα αντίτυπο με ένα έργο που εξετάζει ή κρίνει ένα περιγραφόμενο αντίτυπο."@el ;
        rdakit:toolkitLabel       "αξιολογείται στο (αντίτυπο)"@el ;
        rdakit:toolkitDefinition  "Ένα έργο που εξετάζει ή κρίνει ένα περιγραφόμενο αντίτυπο."@el ;
        rdfs:label                "és avaluat en (ítem)"@ca ;
        skos:definition           "Relaciona un item amb una obra que examina o jutja un ítem descrit."@ca ;
        rdakit:toolkitLabel       "avaluat en (ítem)"@ca ;
        rdakit:toolkitDefinition  "Obra que examina o jutja un ítem descrit."@ca ;
        reg:name                  "kappaleenArviointi"@fi ;
        rdfs:label                "kappaleen arviointi"@fi ;
        reg:lexicalAlias          <rdaa:kappaleenArviointi.fi> ;
        skos:definition           "Liittää kappaleen teokseen, jota kuvailun kohteena olevan kappaleen tutkiva arviointi koskee."@fi ;
        rdakit:toolkitLabel       "kappaleen arviointi"@fi ;
        rdakit:toolkitDefinition  "Teos, jota kuvailun kohteena olevan kappaleen tutkiva arviointi koskee."@fi ;
        reg:name                  "évaluéDansItem"@fr ;
        reg:lexicalAlias          <http://rdaregistry.info/Elements/i/itemÉvaluéDans.fr> ;
        rdakit:toolkitLabel       "evaluert i (eksemplar)"@no ;
        rdakit:toolkitDefinition  "Et verk som utforsker eller vurderer et eksemplar som beskrives."@no ;
        rdakit:hasElementType     "2" ;
        skos:altLabel             "evaluated in (item)"@en ;
        reg:name                  "Példánybankiértékelve"@hu ;
        rdfs:label                "kiértékelve (példány)"@hu ;
        skos:definition           "Egy példányt hozzákapcsol egy olyan műhöz, amely egy leírt példányt megvizsgál vagy értékel."@hu ;
        rdakit:toolkitLabel       "kiértékelve (példány)"@hu ;
        rdakit:toolkitDefinition  "Egy mű, amely egy leírt példányt vizsgál vagy ítél meg."@hu ;
        skos:altLabel             "évalué dans (item)"@fr .

<http://rdaregistry.info/Elements/i/P40067>
        rdfs:isDefinedBy          <http://rdaregistry.info/Elements/i/> ;
        reg:status                <http://metadataregistry.org/uri/RegStatus/1001> ;
        rdf:type                  rdf:Property ;
        reg:name                  "itemReviewedIn"@en ;
        rdfs:label                "is item reviewed in"@en ;
        reg:lexicalAlias          <http://rdaregistry.info/Elements/i/itemReviewedIn.en> ;
        skos:definition           "Relates an item to a work that contains a brief evaluation of an item."@en ;
        rdfs:domain               <http://rdaregistry.info/Elements/c/C10003> ;
        reg:hasUnconstrained      <http://rdaregistry.info/Elements/u/P60211> ;
        rdakit:toolkitLabel       "item reviewed in"@en ;
        rdakit:toolkitDefinition  "A work that contains a brief evaluation of an item."@en ;
        rdfs:label                "est un item recensé dans"@fr ;
        skos:definition           "Met un item en relation avec une œuvre qui contient une brève évaluation d’un item."@fr ;
        rdakit:toolkitLabel       "item recensé dans"@fr ;
        rdakit:toolkitDefinition  "Œuvre qui contient une brève évaluation d’un item."@fr ;
        rdakit:toolkitLabel       "reseñada en (ítem)"@es ;
        rdakit:toolkitDefinition  "Una obra que contiene una evaluación breve del ítem descrito."@es ;
        rdfs:subPropertyOf        <http://rdaregistry.info/Elements/i/P40062> ;
        rdakit:instructionNumber  "23.5" ;
        reg:hasSubproperty        <http://rdaregistry.info/Elements/i/object/P40067> ;
        reg:name                  "đượcTổngQuanTrongBản"@vi ;
        rdfs:label                "được tổng quan trong (bản)"@vi ;
        skos:definition           "Liên kết bản với tác phẩm có chứa đánh giá vắn tắt về bản đang được mô tả."@vi ;
        rdakit:toolkitLabel       "được tổng quan trong (bản)"@vi ;
        rdakit:toolkitDefinition  "Tác phẩm có chứa đánh giá vắn tắt về bản đang được mô tả."@vi ;
        reg:name                  "anmeldtIEksemplar"@da ;
        rdfs:label                "er anmeldt i (eksemplar)"@da ;
        reg:lexicalAlias          <http://rdaregistry.info/Elements/i/anmeldtIEksemplar.da> ;
        skos:definition           "Relaterer et eksemplar til et værk, der indeholder en kort kritik af et beskrevete eksemplar."@da ;
        rdakit:toolkitLabel       "anmeldt i (eksemplar)"@da ;
        rdakit:toolkitDefinition  "Værk der indeholder en kort kritik af et beskrevet eksemplar."@da ;
        rdfs:label                "ist rezensiert in (Exemplar)"@de ;
        skos:definition           "Setzt ein Exemplar mit einem Werk, das eine kurze Untersuchung eines beschriebenen Exemplars enthält, in Beziehung."@de ;
        rdakit:toolkitLabel       "Rezensiert in (Exemplar)"@de ;
        rdakit:toolkitDefinition  "Ein Werk, das eine kurze Untersuchung eines beschriebenen Exemplars enthält."@de ;
        reg:name                  "εξετάζεταιΣτοΑντίτυπο"@el ;
        rdfs:label                "εξετάζεται στο (αντίτυπο)"@el ;
        reg:lexicalAlias          <http://rdaregistry.info/Elements/i/εξετάζεταιΣτοΑντίτυπο.el> ;
        skos:definition           "Συνδέει ένα αντίτυπο με ένα έργο που περιέχει μια σύντομη αξιολόγηση ενός περιγραφόμενου αντιτύπου."@el ;
        rdakit:toolkitLabel       "εξετάζεται στο (αντίτυπο)"@el ;
        rdakit:toolkitDefinition  "Ένα έργο που περιέχει μια σύντομη αξιολόγηση ενός περιγραφόμενου αντιτύπου."@el ;
        rdfs:label                "és revisat en (ítem)"@ca ;
        skos:definition           "Relaciona un item amb una obra que inclou una avaluació breu d’un ítem descrit."@ca ;
        rdakit:toolkitLabel       "revisat en (ítem)"@ca ;
        rdakit:toolkitDefinition  "Obra que inclou una avaluació breu d’un ítem descrit."@ca ;
        reg:name                  "kappaleenArvostelu"@fi ;
        rdfs:label                "kappaleen arvostelu"@fi ;
        reg:lexicalAlias          <rdaa:kappaleenArvostelu.fi> ;
        skos:definition           "Liittää kappaleen teokseen, joka sisältää lyhyen arvostelun kuvailun kohteena olevasta kappalesta"@fi ;
        rdakit:toolkitLabel       "kappaleen arvostelu"@fi ;
        rdakit:toolkitDefinition  "Teos, joka sisältää lyhyen arvostelun kuvailun kohteena olevasta kappaleesta."@fi ;
        reg:name                  "recenséDansItem"@fr ;
        reg:lexicalAlias          <http://rdaregistry.info/Elements/i/itemRecenséDans.fr> ;
        rdakit:toolkitLabel       "anmeldt i (eksemplar)"@no ;
        rdakit:toolkitDefinition  "Et verk som inneholder en kortfattet evaluering av et eksemplar som beskrives."@no ;
        rdakit:hasElementType     "2" ;
        skos:altLabel             "reviewed in (item)"@en ;
        reg:name                  "Példánybanátnézve"@hu ;
        rdfs:label                "átnézve (példány)"@hu ;
        skos:definition           "Egy példányt hozzákapcsol egy olyan műhöz, amely egy leírt példány rövid értékelését tartalmazza."@hu ;
        rdakit:toolkitLabel       "átnézve (példány)"@hu ;
        rdakit:toolkitDefinition  "Egy mű, amely egy leírt példány rövid értékelését tartalmazza."@hu ;
        skos:altLabel             "recensé dans (item)"@fr .

<http://rdaregistry.info/Elements/i/P40002>
        rdfs:isDefinedBy  <http://rdaregistry.info/Elements/i/> ;
        reg:status        <http://metadataregistry.org/uri/RegStatus/1008> .

<http://rdaregistry.info/Elements/i/P40049>
        rdfs:isDefinedBy          <http://rdaregistry.info/Elements/i/> ;
        reg:status                <http://metadataregistry.org/uri/RegStatus/1001> ;
        reg:name                  "manifestationExemplified"@en ;
        rdfs:label                "has manifestation exemplified"@en ;
        skos:definition           "Relates an item to a manifestation that is exemplified by an item."@en ;
        rdf:type                  rdf:Property ;
        rdfs:domain               <http://rdaregistry.info/Elements/c/C10003> ;
        reg:lexicalAlias          <http://rdaregistry.info/Elements/i/manifestationExemplified.en> ;
        rdakit:instructionNumber  "17.12" ;
        rdakit:toolkitLabel       "manifestation exemplified"@en ;
        rdakit:toolkitDefinition  "A manifestation that is exemplified by an item."@en ;
        rdfs:label                "a pour manifestation représentée"@fr ;
        skos:definition           "Met un item en relation avec une manifestation qui est représentée par un item."@fr ;
        rdakit:toolkitLabel       "manifestation représentée"@fr ;
        rdakit:toolkitDefinition  "Manifestation qui est représentée par un item."@fr ;
        rdakit:toolkitLabel       "manifestación ejemplificada"@es ;
        rdakit:toolkitDefinition  "La manifestación ejemplificada en un ítem."@es ;
        rdfs:label                "har exemplar av manifestationen"@sv ;
        rdakit:toolkitLabel       "exemplar av manifestation"@sv ;
        reg:hasSubproperty        <http://rdaregistry.info/Elements/i/object/P40049> ;
        reg:name                  "biểuThịĐượcThểHiện"@vi ;
        rdfs:label                "có biểu thị được ví dụ"@vi ;
        skos:definition           "Liên kết bản với biểu thị được thể hiện bởi bản."@vi ;
        rdakit:toolkitLabel       "biểu thị được thể hiện"@vi ;
        rdakit:toolkitDefinition  "Biểu thị được thể hiện bởi bản."@vi ;
        reg:name                  "eksemplificeretManifestation"@da ;
        rdfs:label                "har eksemplificeret manifestation"@da ;
        reg:lexicalAlias          <http://rdaregistry.info/Elements/i/eksemplificeretManifestation.da> ;
        skos:definition           "Relaterer et eksemplar til en manifestation eksemplificeret af et eksemplar."@da ;
        rdakit:toolkitLabel       "eksemplificeret manifestation"@da ;
        rdakit:toolkitDefinition  "Manifestation eksemplificeret af et eksemplar."@da ;
        rdfs:label                "hat im Exemplar vorliegende Manifestation"@de ;
        skos:definition           "Setzt ein Exemplar mit einer Manifestation, die durch ein Exemplar beispielhaft dargestellt wird, in Beziehung."@de ;
        rdakit:toolkitLabel       "Im Exemplar vorliegende Manifestation"@de ;
        rdakit:toolkitDefinition  "Die Manifestation, die durch ein Exemplar beispielhaft dargestellt wird."@de ;
        reg:name                  "εκδήλωσηΥλοποιημένη"@el ;
        rdfs:label                "έχει υλοποιημένη εκδήλωση"@el ;
        reg:lexicalAlias          <http://rdaregistry.info/Elements/i/εκδήλωσηΥλοποιημένη.el> ;
        skos:definition           "Συνδέει ένα αντίτυπο με μια εκδήλωση που υλοποιείται από ένα αντίτυπο."@el ;
        rdakit:toolkitLabel       "υλοποιημένη εκδήλωση"@el ;
        rdakit:toolkitDefinition  "Μια εκδήλωση που υλοποιείται από ένα αντίτυπο."@el ;
        rdfs:label                "té com a manifestació exemplificada"@ca ;
        skos:definition           "Relaciona un item amb una manifestació exemplificada per un ítem."@ca ;
        rdakit:toolkitLabel       "manifestació exemplificada"@ca ;
        rdakit:toolkitDefinition  "Manifestació exemplificada per un ítem."@ca ;
        reg:name                  "kappaleenEdustamaManifestaatio"@fi ;
        rdfs:label                "kappaleen edustama manifestaatio"@fi ;
        reg:lexicalAlias          <rdaa:kappaleenEdustamaManifestaatio.fi> ;
        skos:definition           "Liittää kappaleen manifestaatioon, jota yksittäinen kappale edustaa."@fi ;
        rdakit:toolkitLabel       "kappaleen edustama manifestaatio"@fi ;
        rdakit:toolkitDefinition  "Manifestaatio, jota yksittäinen kappale edustaa."@fi ;
        reg:name                  "manifestationReprésentée"@fr ;
        reg:lexicalAlias          <http://rdaregistry.info/Elements/i/manifestationReprésentée.fr> ;
        rdakit:toolkitLabel       "eksemplifisering av en manifestasjon"@no ;
        rdakit:toolkitDefinition  "En manifestasjonen eksemplifisert ved et eksemplar."@no ;
        rdfs:subPropertyOf        <http://rdaregistry.info/Elements/i/P40071> ;
        rdakit:hasElementType     "3" ;
        reg:name                  "Szemléltetettmegjelenésiforma"@hu ;
        rdfs:label                "van megjelenési forma példája"@hu ;
        skos:definition           "Egy példányt hozzákapcsol egy megjelenési formához, amelyet egy példány szemléltet."@hu ;
        rdakit:toolkitLabel       "megjelenési forma példája"@hu ;
        rdakit:toolkitDefinition  "Egy példány által szemléltetett megjelenési forma."@hu .

<http://rdaregistry.info/Elements/i/P40023>
        rdfs:isDefinedBy          <http://rdaregistry.info/Elements/i/> ;
        reg:status                <http://metadataregistry.org/uri/RegStatus/1008> ;
        reg:name                  "otherAgentItem"@en ;
        rdfs:label                "has other agent associated with item (Deprecated)"@en ;
        skos:definition           "Relates an item to an agent other than an owner or custodian who is associated with an item. (Deprecated)"@en ;
        rdf:type                  rdf:Property ;
        rdfs:domain               <http://rdaregistry.info/Elements/c/C10003> ;
        reg:hasSubproperty        <http://rdaregistry.info/Elements/i/P40012> ;
        reg:hasSubproperty        <http://rdaregistry.info/Elements/i/P40013> ;
        reg:hasSubproperty        <http://rdaregistry.info/Elements/i/P40014> ;
        reg:hasSubproperty        <http://rdaregistry.info/Elements/i/P40015> ;
        reg:hasSubproperty        <http://rdaregistry.info/Elements/i/P40016> ;
        reg:hasSubproperty        <http://rdaregistry.info/Elements/i/P40017> ;
        reg:hasSubproperty        <http://rdaregistry.info/Elements/i/P40022> ;
        reg:hasSubproperty        <http://rdaregistry.info/Elements/i/P40024> ;
        reg:hasSubproperty        <http://rdaregistry.info/Elements/i/P40025> ;
        reg:lexicalAlias          <http://rdaregistry.info/Elements/i/otherAgentItem.en> ;
        reg:hasUnconstrained      <http://rdaregistry.info/Elements/u/P60374> ;
        rdakit:instructionNumber  "22.4" ;
        rdakit:toolkitLabel       "other agent associated with item (Deprecated)"@en ;
        rdakit:toolkitDefinition  "An agent other than an owner or custodian who is associated with an item. (Deprecated)"@en ;
        rdfs:label                "a pour autre agent associé à un item"@fr ;
        skos:definition           "Met un item en relation avec un agent, autre qu’un propriétaire ou un dépositaire, associé à un item."@fr ;
        skos:scopeNote            "Sont inclus les conservateurs, les relieurs, les restaurateurs, etc."@fr ;
        rdakit:toolkitLabel       "autre agent associé à un item"@fr ;
        rdakit:toolkitDefinition  "Agent, autre qu’un propriétaire ou un dépositaire, associé à un item."@fr ;
        rdakit:toolkitLabel       "otra persona, familia o entidad corporativa asociada con un ítem"@es ;
        rdakit:toolkitDefinition  "Una persona, familia o entidad corporativa (diferente a un propietario o custodio), asociada con un ítem."@es ;
        skos:scopeNote            "Curators, binders, restorationists, etc., are included. (Deprecated)"@en ;
        rdfs:label                "har övrig person, familj/släkt eller institution knuten till ett exemplar"@sv ;
        rdakit:toolkitLabel       "övrig person, familj/släkt eller institution knuten till ett exemplar"@sv ;
        reg:hasSubproperty        <http://rdaregistry.info/Elements/i/object/P40023> ;
        rdfs:subPropertyOf        <http://rdaregistry.info/Elements/i/P40072> ;
        reg:name                  "tácNhânKhácCủaBản"@vi ;
        rdfs:label                "có tác nhân khác của bản"@vi ;
        skos:definition           "Liên kết bản với tác nhân liên quan tới bản, khác với người chủ hoặc người giám hộ."@vi ;
        skos:scopeNote            "Người trông nom, người đóng sách, người phục chế, v.v..., được bao gồm."@vi ;
        rdakit:toolkitLabel       "tác nhân khác của bản"@vi ;
        rdakit:toolkitDefinition  "Tác nhân liên quan tới bản, khác với người chủ hoặc người giám hộ."@vi ;
        reg:name                  "andenPFCEksemplar"@da ;
        rdfs:label                "har anden person, familie eller korporation knyttet til et eksemplar"@da ;
        reg:lexicalAlias          <http://rdaregistry.info/Elements/i/andenPFCEksemplar.da> ;
        skos:definition           "Relaterer et eksemplar til en agent bortset fra en ejer eller forvalter, der er knyttet til et eksemplar."@da ;
        skos:scopeNote            "Kuratorer, bogbindere, konservatorer etc, er omfattet."@da ;
        rdakit:toolkitLabel       "anden agent knyttet til et eksemplar"@da ;
        rdakit:toolkitDefinition  "Agent bortset fra en ejer eller forvalter, der er knyttet til et eksemplar."@da ;
        rdfs:label                "hat sonstigen Akteur, der mit einem Exemplar in Verbindung steht"@de ;
        skos:definition           "Setzt ein Exemplar mit einem Akteur, der mit einem Exemplar in Verbindung steht, aber nicht der Eigentümer oder der Verwahrer ist, in Beziehung."@de ;
        skos:scopeNote            "Dazu gehören Kuratoren, Buchbinder, Restauratoren usw."@de ;
        rdakit:toolkitLabel       "Sonstiger Akteur der mit einem Exemplar in Verbindung steht"@de ;
        rdakit:toolkitDefinition  "Ein Akteur, der mit einem Exemplar in Verbindung steht, aber nicht der Eigentümer oder der Verwahrer ist."@de ;
        reg:name                  "άλλοςΦορέαςΑντιτύπου"@el ;
        rdfs:label                "έχει άλλον φορέα συνδεδεμένο με το αντίτυπο"@el ;
        reg:lexicalAlias          <http://rdaregistry.info/Elements/i/άλλοςΦορέαςΑντιτύπου.el> ;
        skos:definition           "Συνδέει ένα αντίτυπο με έναν φορέα άλλον από τον ιδιοκτήτη ή τον θεματοφύλακα ο οποίος συνδέεται με ένα αντίτυπο."@el ;
        skos:scopeNote            "Περιλαμβάνονται επιμελητές έκθεσης, βιβλιοδέτες, συντηρητές κ.λπ."@el ;
        rdakit:toolkitLabel       "άλλος φορέας συνδεδεμένος με το αντίτυπο"@el ;
        rdakit:toolkitDefinition  "Ένας φορέας άλλος από τον ιδιοκτήτη ή τον θεματοφύλακα ο οποίος συνδέεται με ένα αντίτυπο."@el ;
        rdfs:label                "té com a altre agent associat amb un ítem"@ca ;
        skos:definition           "Relaciona un item amb un agent diferent d’un propietari o un dipositari associat amb un ítem."@ca ;
        skos:scopeNote            "Inclou els conservadors, els enquadernadors, els restauradors, etc."@ca ;
        rdakit:toolkitLabel       "altre agent associat amb un ítem"@ca ;
        rdakit:toolkitDefinition  "Agent diferent d’un propietari o un dipositari associat amb un ítem."@ca ;
        reg:name                  "kappaleeseenLiittyvaMuuToimija"@fi ;
        rdfs:label                "kappaleeseen liittyvä muu toimija"@fi ;
        reg:lexicalAlias          <rdaa:kappaleeseenLiittyvaMuuToimija.fi> ;
        skos:definition           "Liittää kappaleen muuhun toimijaan, joka ei ole kappaleen omistaja tai säilyttäjä."@fi ;
        skos:scopeNote            "Kappaleeseen liittyviin muihin toimijoihin kuuluvat kuraattorit, kirjansitojat, restauroijat jne."@fi ;
        rdakit:toolkitLabel       "kappaleeseen liittyvä muu toimija"@fi ;
        rdakit:toolkitDefinition  "Kappaleeseen liittyvä muu toimija, joka ei ole kappaleen omistaja tai säilyttäjä."@fi ;
        reg:name                  "autreAgentAssociéÀUnItem"@fr ;
        reg:lexicalAlias          <http://rdaregistry.info/Elements/i/autreAgentAssociéÀUnItem.fr> ;
        rdakit:toolkitLabel       "annen agent som forbindes med eksemplar"@no ;
        rdakit:toolkitDefinition  "En agent som forbindes med et eksemplar og som ikke er en eier eller oppbevarer."@no ;
        rdakit:hasElementType     "3" ;
        reg:name                  "máspéldányÁgens"@hu ;
        rdfs:label                "van más, a példányhoz kötődő ágense"@hu ;
        skos:definition           "Egy példányt hozzákapcsol egy ágenshez (személyhez, családhoz vagy testülethez), aki/amely más, mint a példányhoz kötődő tulajdonos vagy őrző."@hu ;
        skos:scopeNote            "Kurátorok, könyvkötők, restaurátorok stb. beletartoznak."@hu ;
        rdakit:toolkitLabel       "példányhoz kötődő másik ágens"@hu ;
        rdakit:toolkitDefinition  "Egy ágens (személy, család vagy testület), aki/amely nem a tulajdonos vagy az őrző, aki/amely kötődik egy példányhoz."@hu ;
        reg:hasSubproperty        <http://rdaregistry.info/Elements/i/P40093> .

<http://rdaregistry.info/Elements/i/P40003>
        rdfs:isDefinedBy          <http://rdaregistry.info/Elements/i/> ;
        reg:status                <http://metadataregistry.org/uri/RegStatus/1001> ;
        reg:name                  "modificationOfItem"@en ;
        rdfs:label                "has modification of item"@en ;
        skos:definition           "Relates an item to a modification that is specific to an item and is assumed not to apply to other items exemplifying the same manifestation."@en ;
        rdf:type                  rdf:Property ;
        rdfs:domain               <http://rdaregistry.info/Elements/c/C10003> ;
        reg:lexicalAlias          <http://rdaregistry.info/Elements/i/modificationOfItem.en> ;
        reg:hasUnconstrained      <http://rdaregistry.info/Elements/u/P60056> ;
        rdakit:instructionNumber  "3.22" ;
        rdakit:toolkitLabel       "modification of item"@en ;
        rdakit:toolkitDefinition  "A modification that is specific to an item and is assumed not to apply to other items exemplifying the same manifestation."@en ;
        rdfs:label                "a pour modification d’un item"@fr ;
        skos:definition           "Met un item en relation avec une modification qui est particulière à un item et qui est censée ne pas concerner les autres items représentant la même manifestation."@fr ;
        rdakit:toolkitLabel       "modification d’un item"@fr ;
        rdakit:toolkitDefinition  "Modification qui est particulière à un item et qui est censée ne pas concerner les autres items représentant la même manifestation."@fr ;
        rdakit:toolkitLabel       "nota sobre la característica del soporte de ítem específico"@es ;
        rdakit:toolkitDefinition  "Una nota que proporciona información sobre las características del soporte que son específicas al ítem descrito y se asume que no aplican a otros ítems que ejemplifican la misma manifestación."@es ;
        reg:hasSubproperty        <http://rdaregistry.info/Elements/i/P40010> ;
        reg:hasSubproperty        <http://rdaregistry.info/Elements/i/P40011> ;
        reg:hasSubproperty        <http://rdaregistry.info/Elements/i/object/P40003> ;
        rdfs:label                "har anmärkning om exemplarspecifika bäraregenskaper"@sv ;
        rdakit:toolkitLabel       "anmärkning om exemplarspecifika bäraregenskaper"@sv ;
        reg:name                  "ghiChúĐặcTrưngVậtMangBảnCụThể"@vi ;
        rdfs:label                "có ghi chú đặc trưng vật mang bản cụ thể"@vi ;
        skos:definition           "Liên kết bản với ghi chú cung cấp thông tin phụ trợ về đặc trưng vật mang tin đối với bản cụ thể đang được mô tả và được thừa nhận không áp dụng đối với các bản khác sao chép từ cùng biểu thị."@vi ;
        rdakit:toolkitLabel       "ghi chú đặc trưng vật mang bản cụ thể"@vi ;
        rdakit:toolkitDefinition  "Ghi chú cung cấp thông tin phụ trợ về đặc trưng vật mang tin đối với bản cụ thể đang được mô tả và được thừa nhận không áp dụng đối với các bản khác sao chép từ cùng biểu thị."@vi ;
        reg:name                  "noteOmEksemplarspecifikeBærerkarakteristika"@da ;
        rdfs:label                "har note om eksemplarspecifike bærerkarakteristika"@da ;
        reg:lexicalAlias          <http://rdaregistry.info/Elements/i/noteOmEksemplarspecifikeBærerkarakteristika.da> ;
        skos:definition           "Relaterer et eksemplar til en note, der giver supplerende oplysninger om bærerkarakteristika, der er specifikke for det eksemplar, der beskrives, og som ikke gælder andre eksemplarer af manifestationen."@da ;
        rdakit:toolkitLabel       "note om eksemplarspecifike bærerkarakteristika"@da ;
        rdakit:toolkitDefinition  "Note, der giver supplerende oplysninger om bærerkarakteristika, der er specifikke for det eksemplar, der beskrives, og som ikke gælder andre eksemplarer af manifestationen."@da ;
        rdfs:label                "hat Anmerkung zu einer exemplarspezifischen Datenträgereigenschaft"@de ;
        skos:definition           "Setzt ein Exemplar mit einer Anmerkung, die zusätzliche Informationen über Datenträgereigenschaften liefert, die spezifisch für ein Exemplar sind, das beschrieben wird, und von denen man annimmt, dass sie nicht auf andere Exemplare zutreffen, die dieselbe Manifestation verkörpern, in Beziehung."@de ;
        rdakit:toolkitLabel       "Anmerkung zu einer exemplarspezifischen Datenträgereigenschaft"@de ;
        rdakit:toolkitDefinition  "Eine Anmerkung, die zusätzliche Informationen über Datenträgereigenschaften liefert, die spezifisch für ein Exemplar sind, das beschrieben wird, und von denen man annimmt, dass sie nicht auf andere Exemplare zutreffen, die dieselbe Manifestation verkörpern."@de ;
        reg:name                  "σημείωσηΣτοΣυγκεκριμένοΑντίτυποΤωνΧαρακτηριστικώνΤουΦορέαΑποθήκευσης"@el ;
        rdfs:label                "έχει σημείωση σε συγκεκριμένο αντίτυπο των χαρακτηριστικών του φορέα αποθήκευσης"@el ;
        reg:lexicalAlias          <http://rdaregistry.info/Elements/i/σημείωσηΣτοΣυγκεκριμένοΑντίτυποΤωνΧαρακτηριστικώνΤουΦορέαΑποθήκευσης.el> ;
        skos:definition           "Συνδέει ένα αντίτυπο με μια σημείωση που παρέχει πρόσθετες πληροφορίες σχετικά με τα χαρακτηριστικά του φορέα αποθήκευσης, τα οποία αναφέρονται σε ένα συγκεκριμένο περιγραφόμενο αντίτυπο και θεωρούνται ότι δεν βρίσκουν εφαρμογή σε άλλα αντίτυπα τα οποία υλοποιούν την ίδια εκδήλωση."@el ;
        rdakit:toolkitLabel       "σημείωση σε συγκεκριμένο αντίτυπο των χαρακτηριστικών του φορέα αποθήκευσης"@el ;
        rdakit:toolkitDefinition  "Μια σημείωση που παρέχει πρόσθετες πληροφορίες σχετικά με τα χαρακτηριστικά του φορέα αποθήκευσης, τα οποία αναφέρονται σε ένα συγκεκριμένο περιγραφόμενο αντίτυπο και θεωρούνται ότι δεν βρίσκουν εφαρμογή σε άλλα αντίτυπα τα οποία υλοποιούν την ίδια εκδήλωση."@el ;
        rdfs:label                "té com a nota sobre característiques de suport físic específiques d’un ítem concret"@ca ;
        skos:definition           "Relaciona un item amb una nota que proporciona la informació addicional sobre les característiques del suport físic que són específiques d’un ítem que es descriu i que se suposa que no s’apliquen als altres ítems que exemplifiquen la mateixa manifestació."@ca ;
        rdakit:toolkitLabel       "nota sobre característiques de suport físic específiques d’un ítem concret"@ca ;
        rdakit:toolkitDefinition  "Nota que proporciona la informació addicional sobre les característiques del suport físic que són específiques d’un ítem que es descriu i que se suposa que no s’apliquen als altres ítems que exemplifiquen la mateixa manifestació."@ca ;
        reg:name                  "huomautusKappalekohtaisenTallenteenOminaisuudesta"@fi ;
        rdfs:label                "huomautus kappalekohtaisen tallenteen ominaisuudesta"@fi ;
        reg:lexicalAlias          <rdaa:huomautusKappalekohtaisenTallenteenOminaisuudesta.fi> ;
        skos:definition           "Liittää kappaleen huomautukseen, joka antaa lisätietoa kuvailun kohteena olevan kappaleen tallenteen eritysipiirteistä. Erityispiirteiden ei oleteta koskevan samaa manifestaatiota edustavia muita kappaleita."@fi ;
        rdakit:toolkitLabel       "huomautus kappalekohtaisen tallenteen ominaisuudesta"@fi ;
        rdakit:toolkitDefinition  "Huomautus, joka antaa lisätietoa kuvailun kohteena olevan kappaleen tallenteen eritysipiirteistä. Erityispiirteiden ei oleteta koskevan samaa manifestaatiota edustavia muita kappaleita."@fi ;
        reg:name                  "noteSurLesCaractéristiquesDuSupportMatérielDunItemParticulier"@fr ;
        reg:lexicalAlias          <http://rdaregistry.info/Elements/i/modificationDunItem.fr> ;
        rdakit:toolkitLabel       "note om eksemplarspesifikke kjennetegn"@no ;
        rdakit:toolkitDefinition  "En note som gir ytterligere informasjon om bæreregenskaper som er spesifikke for et eksemplar som beskrives og som antas å ikke gjelde andre eksemplarer av samme manifestasjon."@no ;
        rdakit:hasElementType     "6" ;
        reg:name                  "megjegyzésPéldánySpecifikusHordozóJellemzőről"@hu ;
        rdfs:label                "van megjegyzése példányspecifikus hordozójellemzőről"@hu ;
        skos:definition           "Egy példányt hozzákapcsol egy olyan megjegyzéshez, amely további információkat nyújt a hordozó jellemzőiről, amelyek az éppen leírt példány sajátosságai és amelyek feltehetően nem alkalmazhatók olyan más példányokra, amelyek ugyanazt a megjelenési formát példázzák."@hu ;
        rdakit:toolkitLabel       "megjegyzés példányspecifikus hordozójellemzőről"@hu ;
        rdakit:toolkitDefinition  "Megjegyzés, amely további információkat közöl olyan hordozói ismérvekről, amelyek egy éppen leírt példányra jellemzők és feltehetően nem alkalmazhatók olyan más példányokra, amelyek ugyanazt a megjelenési formátumot példázzák."@hu ;
        skos:altLabel             "note on item-specific carrier characteristic"@en ;
        reg:hasSubproperty        <http://rdaregistry.info/Elements/i/datatype/P40003> ;
        rdfs:subPropertyOf        <http://rdaregistry.info/Elements/i/P40028> ;
        skos:altLabel             "note sur les caractéristiques du support matériel d’un item particulier"@fr .

<http://rdaregistry.info/Elements/i/P40093>
        rdfs:isDefinedBy          <http://rdaregistry.info/Elements/i/> ;
        reg:status                <http://metadataregistry.org/uri/RegStatus/1001> ;
        rdfs:label                "has modifier agent"@en ;
        rdf:type                  rdf:Property ;
        reg:name                  "modifierAgent"@en ;
        reg:lexicalAlias          <http://rdaregistry.info/Elements/i/modifierAgent.en> ;
        rdfs:domain               <http://rdaregistry.info/Elements/c/C10003> ;
        rdakit:hasElementType     "2" ;
        rdakit:toolkitLabel       "modifier agent"@en ;
        skos:definition           "Relates an item to an agent that makes changes to an item without creating a new manifestation."@en ;
        rdakit:toolkitDefinition  "An agent who makes changes to an item without creating a new manifestation."@en ;
        reg:hasUnconstrained      <http://rdaregistry.info/Elements/u/P61031> ;
        rdfs:subPropertyOf        <http://rdaregistry.info/Elements/i/P40072> ;
        reg:hasSubproperty        <http://rdaregistry.info/Elements/i/datatype/P40093> ;
        skos:altLabel             "modifier"@en ;
        rdfs:label                "a pour agent modificateur"@fr ;
        skos:definition           "Met un item en relation avec un agent qui apporte des modifications à un item sans créer une nouvelle manifestation."@fr ;
        skos:altLabel             "modificateur"@fr ;
        rdakit:toolkitLabel       "agent modificateur"@fr ;
        rdakit:toolkitDefinition  "Agent qui apporte des modifications à un item sans créer une nouvelle manifestation."@fr ;
        reg:lexicalAlias          <http://rdaregistry.info/Elements/i/agentModificateur.fr> .

<http://rdaregistry.info/Elements/i/P40128>
        rdfs:isDefinedBy          <http://rdaregistry.info/Elements/i/> ;
        reg:status                <http://metadataregistry.org/uri/RegStatus/1001> ;
        rdfs:label                "has modifier collective agent"@en ;
        reg:lexicalAlias          <http://rdaregistry.info/Elements/i/modifierCollectiveAgent.en> ;
        skos:definition           "Relates an item to a collective agent that makes changes to an item without creating a new manifestation."@en ;
        rdakit:toolkitLabel       "modifier collective agent"@en ;
        rdakit:toolkitDefinition  "A collective agent who makes changes to an item without creating a new manifestation."@en ;
        rdf:type                  rdf:Property ;
        reg:name                  "modifierCollectiveAgent" ;
        rdfs:domain               <http://rdaregistry.info/Elements/c/C10003> ;
        rdakit:hasElementType     "2" ;
        reg:hasSubproperty        <http://rdaregistry.info/Elements/i/datatype/P40128> ;
        reg:hasSubproperty        <http://rdaregistry.info/Elements/i/object/P40128> ;
        rdfs:subPropertyOf        <http://rdaregistry.info/Elements/i/P40076> ;
        rdfs:subPropertyOf        <http://rdaregistry.info/Elements/i/P40093> ;
        reg:hasSubproperty        <http://rdaregistry.info/Elements/i/P40144> ;
        reg:hasSubproperty        <http://rdaregistry.info/Elements/i/P40160> ;
        reg:hasUnconstrained      <http://rdaregistry.info/Elements/u/P61031> ;
        rdfs:label                "a pour agent collectif modificateur"@fr ;
        skos:definition           "Met un item en relation avec un agent collectif qui apporte des modifications à un item sans créer une nouvelle manifestation."@fr ;
        rdakit:toolkitLabel       "agent collectif modificateur"@fr ;
        rdakit:toolkitDefinition  "Agent collectif qui apporte des modifications à un item sans créer une nouvelle manifestation."@fr ;
        reg:lexicalAlias          <http://rdaregistry.info/Elements/i/agentCollectifModificateur.fr> .

<http://rdaregistry.info/Elements/i/P40144>
        rdfs:isDefinedBy          <http://rdaregistry.info/Elements/i/> ;
        reg:status                <http://metadataregistry.org/uri/RegStatus/1001> ;
        rdfs:label                "has modifier corporate body"@en ;
        reg:lexicalAlias          <http://rdaregistry.info/Elements/i/modifierCorporateBody.en> ;
        skos:definition           "Relates an item to a corporate body that makes changes to an item without creating a new manifestation."@en ;
        rdakit:toolkitLabel       "modifier corporate body"@en ;
        rdakit:toolkitDefinition  "A corporate body who makes changes to an item without creating a new manifestation."@en ;
        rdf:type                  rdf:Property ;
        reg:name                  "modifierCorporateBody" ;
        rdfs:domain               <http://rdaregistry.info/Elements/c/C10003> ;
        rdakit:hasElementType     "2" ;
        reg:hasSubproperty        <http://rdaregistry.info/Elements/i/datatype/P40144> ;
        reg:hasSubproperty        <http://rdaregistry.info/Elements/i/object/P40144> ;
        rdfs:subPropertyOf        <http://rdaregistry.info/Elements/i/P40075> ;
        rdfs:subPropertyOf        <http://rdaregistry.info/Elements/i/P40128> ;
        reg:hasUnconstrained      <http://rdaregistry.info/Elements/u/P61031> ;
        rdfs:label                "a pour collectivité modificatrice"@fr ;
        skos:definition           "Met un item en relation avec une collectivité qui apporte des modifications à un item sans créer une nouvelle manifestation."@fr ;
        rdakit:toolkitLabel       "collectivité modificatrice"@fr ;
        rdakit:toolkitDefinition  "Collectivité qui apporte des modifications à un item sans créer une nouvelle manifestation."@fr ;
        reg:lexicalAlias          <http://rdaregistry.info/Elements/i/collectivitéModificatrice.fr> .

<http://rdaregistry.info/Elements/i/P40160>
        rdfs:isDefinedBy          <http://rdaregistry.info/Elements/i/> ;
        reg:status                <http://metadataregistry.org/uri/RegStatus/1001> ;
        rdfs:label                "has modifier family"@en ;
        reg:lexicalAlias          <http://rdaregistry.info/Elements/i/modifierFamily.en> ;
        skos:definition           "Relates an item to a family that makes changes to an item without creating a new manifestation."@en ;
        rdakit:toolkitLabel       "modifier family"@en ;
        rdakit:toolkitDefinition  "A family who makes changes to an item without creating a new manifestation."@en ;
        rdf:type                  rdf:Property ;
        reg:name                  "modifierFamily" ;
        rdfs:domain               <http://rdaregistry.info/Elements/c/C10003> ;
        rdakit:hasElementType     "2" ;
        reg:hasSubproperty        <http://rdaregistry.info/Elements/i/datatype/P40160> ;
        reg:hasSubproperty        <http://rdaregistry.info/Elements/i/object/P40160> ;
        rdfs:subPropertyOf        <http://rdaregistry.info/Elements/i/P40074> ;
        rdfs:subPropertyOf        <http://rdaregistry.info/Elements/i/P40128> ;
        reg:hasUnconstrained      <http://rdaregistry.info/Elements/u/P61031> ;
        rdfs:label                "a pour famille modificatrice"@fr ;
        skos:definition           "Met un item en relation avec une famille qui apporte des modifications à un item sans créer une nouvelle manifestation."@fr ;
        rdakit:toolkitLabel       "famille modificatrice"@fr ;
        rdakit:toolkitDefinition  "Famille qui apporte des modifications à un item sans créer une nouvelle manifestation."@fr ;
        reg:lexicalAlias          <http://rdaregistry.info/Elements/i/familleModificatrice.fr> .

<http://rdaregistry.info/Elements/i/P40112>
        rdfs:isDefinedBy          <http://rdaregistry.info/Elements/i/> ;
        reg:status                <http://metadataregistry.org/uri/RegStatus/1001> ;
        rdfs:label                "has modifier person"@en ;
        reg:lexicalAlias          <http://rdaregistry.info/Elements/i/modifierPerson.en> ;
        skos:definition           "Relates an item to a person that makes changes to an item without creating a new manifestation."@en ;
        rdakit:toolkitLabel       "modifier person"@en ;
        rdakit:toolkitDefinition  "A person who makes changes to an item without creating a new manifestation."@en ;
        rdf:type                  rdf:Property ;
        reg:name                  "modifierPerson" ;
        rdfs:domain               <http://rdaregistry.info/Elements/c/C10003> ;
        rdakit:hasElementType     "2" ;
        reg:hasSubproperty        <http://rdaregistry.info/Elements/i/datatype/P40112> ;
        reg:hasSubproperty        <http://rdaregistry.info/Elements/i/object/P40112> ;
        rdfs:subPropertyOf        <http://rdaregistry.info/Elements/i/P40073> ;
        rdfs:subPropertyOf        <http://rdaregistry.info/Elements/i/P40093> ;
        reg:hasUnconstrained      <http://rdaregistry.info/Elements/u/P61031> ;
        rdfs:label                "a pour personne modificatrice"@fr ;
        skos:definition           "Met un item en relation avec une personne qui apporte des modifications à un item sans créer une nouvelle manifestation."@fr ;
        rdakit:toolkitLabel       "personne modificatrice"@fr ;
        rdakit:toolkitDefinition  "Personne qui apporte des modifications à un item sans créer une nouvelle manifestation."@fr ;
        reg:lexicalAlias          <http://rdaregistry.info/Elements/i/personneModificatrice.fr> .

<http://rdaregistry.info/Elements/i/P40010>
        rdfs:isDefinedBy          <http://rdaregistry.info/Elements/i/> ;
        reg:status                <http://metadataregistry.org/uri/RegStatus/1001> ;
        reg:name                  "noteOnDimensionsOfItem"@en ;
        rdfs:label                "has note on dimensions of item"@en ;
        skos:definition           "Relates an item to a note on item that provides information on the dimensions of an item."@en ;
        rdf:type                  rdf:Property ;
        rdfs:domain               <http://rdaregistry.info/Elements/c/C10003> ;
        reg:lexicalAlias          <http://rdaregistry.info/Elements/i/noteOnDimensionsOfItem.en> ;
        reg:hasUnconstrained      <http://rdaregistry.info/Elements/u/P60133> ;
        rdakit:instructionNumber  "3.22.3" ;
        rdakit:toolkitLabel       "note on dimensions of item"@en ;
        rdakit:toolkitDefinition  "A note on item that provides information on the dimensions of an item."@en ;
        rdfs:label                "a pour note sur les dimensions d’un item"@fr ;
        skos:definition           "Met un item en relation avec une note sur un item qui fournit de l’information sur les dimensions d’un item."@fr ;
        rdakit:toolkitLabel       "note sur les dimensions d’un item"@fr ;
        rdakit:toolkitDefinition  "Note sur un item qui fournit de l’information sur les dimensions d’un item."@fr ;
        rdakit:toolkitLabel       "nota sobre dimensiones del ítem"@es ;
        rdakit:toolkitDefinition  "Una nota que proporciona información sobre las dimensiones del ítem específico descrito que no esta registrado como parte del elemento dimensiones."@es ;
        rdfs:subPropertyOf        <http://rdaregistry.info/Elements/i/P40028> ;
        reg:hasSubproperty        <http://rdaregistry.info/Elements/i/object/P40010> ;
        rdfs:label                "har anmärkning om exemplarets mått"@sv ;
        rdakit:toolkitLabel       "anmärkning om exemplarets mått"@sv ;
        reg:name                  "ghiChúVềKíchThướcCủaBản"@vi ;
        rdfs:label                "có ghi chú về kích thước của bản"@vi ;
        skos:definition           "Liên kết bản với ghi chú cung cấp thông tin về kích thước của bản cụ thể đang được mô tả nhưng không được ghi như là phần của yếu tố kích thước."@vi ;
        rdakit:toolkitLabel       "ghi chú về kích thước của bản"@vi ;
        rdakit:toolkitDefinition  "Ghi chú cung cấp thông tin về kích thước của bản cụ thể đang được mô tả nhưng không được ghi như là phần của yếu tố kích thước."@vi ;
        reg:name                  "noteOmEksemplarsStørrelse"@da ;
        rdfs:label                "har note om eksemplars størrelse"@da ;
        reg:lexicalAlias          <http://rdaregistry.info/Elements/i/noteOmEksemplarsStørrelse.da> ;
        skos:definition           "Relaterer et eksemplar til en note, der giver oplysninger om det specifikke eksemplars størrelse, der ikke er registreret som en del af størrelsesangivelsen."@da ;
        rdakit:toolkitLabel       "note om eksemplars størrelse"@da ;
        rdakit:toolkitDefinition  "Note, der giver oplysninger om det specifikke eksemplars størrelse, der ikke er registreret som en del af størrelsesangivelsen."@da ;
        rdfs:label                "hat Anmerkung zu den Maßen des Exemplars"@de ;
        skos:definition           "Setzt ein Exemplar mit einer Anmerkung, die Informationen über die Maße des spezifischen Exemplars liefert, das beschrieben wird, die nicht als Teil des Elements Maße erfasst werden, in Beziehung."@de ;
        rdakit:toolkitLabel       "Anmerkung zu den Maßen des Exemplars"@de ;
        rdakit:toolkitDefinition  "Eine Anmerkung, die Informationen über die Maße des spezifischen Exemplars liefert, das beschrieben wird, die nicht als Teil des Elements Maße erfasst werden."@de ;
        reg:name                  "σημείωσηΣτιςΔιαστάσειςΤουΑντιτύπου"@el ;
        rdfs:label                "έχει σημείωση στις διαστάσεις του αντιτύπου"@el ;
        reg:lexicalAlias          <http://rdaregistry.info/Elements/i/σημείωσηΣτιςΔιαστάσειςΤουΑντιτύπου.el> ;
        skos:definition           "Συνδέει ένα ανίτυπο με μια σημείωση που παρέχει πληροφορίες αναφορικά με τις διαστάσεις ενός συγκεκριμένου περιγραφόμενου αντιτύπου οι οποίες δεν καταχωρίζονται ως μέρος του στοιχείου των διαστάσεων."@el ;
        rdakit:toolkitLabel       "σημείωση στις διαστάσεις του αντιτύπου"@el ;
        rdakit:toolkitDefinition  "Μια σημείωση που παρέχει πληροφορίες αναφορικά με τις διαστάσεις ενός συγκεκριμένου περιγραφόμενου αντιτύπου, οι οποίες δεν καταχωρίζονται ως μέρος του στοιχείου των διαστάσεων."@el ;
        rdfs:label                "té com a nota sobre dimensions d’un ítem"@ca ;
        skos:definition           "Relaciona un item amb una nota que proporciona la informació sobre les dimensions d’un ítem concret que es descriu i que no s’ha enregistrat com a part de l’element Dimensions."@ca ;
        rdakit:toolkitLabel       "nota sobre dimensions d'un ítem"@ca ;
        rdakit:toolkitDefinition  "Nota que proporciona la informació sobre les dimensions d’un ítem concret que es descriu i que no s’ha enregistrat com a part de l’element Dimensions."@ca ;
        reg:name                  "huomautusKappaleenKoosta"@fi ;
        rdfs:label                "huomautus kappaleen koosta"@fi ;
        reg:lexicalAlias          <rdaa:huomautusKappaleenKoosta.fi> ;
        skos:definition           "Liittää kappaleen huomautukseen kuvailun kohteena olevan yksittäisen kappaleen koosta, jota ei merkitä osana varsinaista kokoelementtiä."@fi ;
        rdakit:toolkitLabel       "huomautus kappaleen koosta"@fi ;
        rdakit:toolkitDefinition  "Huomautus kuvailun kohteen olevan yksittäisen kappaleen koosta, jota ei merkitä osana varsinaista kokoelementtiä."@fi ;
        reg:name                  "noteSurLesDimensionsDunItem"@fr ;
        reg:lexicalAlias          <http://rdaregistry.info/Elements/i/noteSurLesDimensionsDunItem.fr> ;
        rdakit:toolkitLabel       "note om eksemplarets størrelse"@no ;
        rdakit:toolkitDefinition  "En note som gir informasjon om størrelsen til et bestemt eksemplar som beskrives, som ikke er registerert som en del av et størrelseselement."@no ;
        rdakit:hasElementType     "6" ;
        reg:name                  "megjegyzésPéldányMéreteiről"@hu ;
        rdfs:label                "van megjegyzése példányméretekről"@hu ;
        skos:definition           "Egy példányt hozzákapcsol egy megjegyzéshez, amely egy éppen leírt sajátos példány méreteiről nyújt információkat, amelyek nincsenek a méretelem részeként rögzítve."@hu ;
        rdakit:toolkitLabel       "megjegyzés példányméretekről"@hu ;
        rdakit:toolkitDefinition  "Megjegyzés, amely egy éppen leírt különleges példány méretarányairól szolgáltat információkat, amelyek nincsenek rögzítve a méretarány elem részeként. "@hu .

<http://rdaregistry.info/Elements/i/P40011>
        rdfs:isDefinedBy          <http://rdaregistry.info/Elements/i/> ;
        reg:status                <http://metadataregistry.org/uri/RegStatus/1001> ;
        reg:name                  "noteOnExtentOfItem"@en ;
        rdfs:label                "has note on extent of item"@en ;
        skos:definition           "Relates an item to a note on item that provides information on the extent of an item."@en ;
        rdf:type                  rdf:Property ;
        rdfs:domain               <http://rdaregistry.info/Elements/c/C10003> ;
        reg:lexicalAlias          <http://rdaregistry.info/Elements/i/noteOnExtentOfItem.en> ;
        reg:hasUnconstrained      <http://rdaregistry.info/Elements/u/P60134> ;
        rdakit:instructionNumber  "3.22.2" ;
        rdakit:toolkitLabel       "note on extent of item"@en ;
        rdakit:toolkitDefinition  "A note on item that provides information on the extent of an item."@en ;
        rdfs:label                "a pour note sur l’étendue d’un item"@fr ;
        skos:definition           "Met un item en relation avec une note sur un item qui fournit de l’information sur l’étendue d’un item."@fr ;
        rdakit:toolkitLabel       "note sur l’étendue d’un item"@fr ;
        rdakit:toolkitDefinition  "Note sur un item qui fournit de l’information sur l’étendue d’un item."@fr ;
        rdakit:toolkitLabel       "nota sobre la extensión del ítem"@es ;
        rdakit:toolkitDefinition  "Una nota que proporciona información sobre la extensión del ítem específico descrito que está registrado como parte del elemento extensión"@es ;
        rdfs:subPropertyOf        <http://rdaregistry.info/Elements/i/P40028> ;
        reg:hasSubproperty        <http://rdaregistry.info/Elements/i/object/P40011> ;
        rdfs:label                "har anmärkning om exemplarets omfång"@sv ;
        rdakit:toolkitLabel       "anmärkning om exemplarets omfång"@sv ;
        reg:name                  "ghiChúVềQuyMôCủaBản"@vi ;
        rdfs:label                "có ghi chú về quy mô của bản"@vi ;
        skos:definition           "Liên kết bản với ghi chú cung cấp thông tin về quy mô của bản cụ thể đang được mô tả nhưng không được ghi như là phần của yếu tố quy mô."@vi ;
        rdakit:toolkitLabel       "ghi chú về quy mô của bản"@vi ;
        rdakit:toolkitDefinition  "Ghi chú cung cấp thông tin về quy mô của bản cụ thể đang được mô tả nhưng không được ghi như là phần của yếu tố quy mô."@vi ;
        reg:name                  "noteOmOmfangAfEksemplar"@da ;
        rdfs:label                "har note om omfang af eksemplar"@da ;
        reg:lexicalAlias          <http://rdaregistry.info/Elements/i/noteOmOmfangAfEksemplar.da> ;
        skos:definition           "Relaterer et eksemplar til en note, der giver oplysninger om det specifikke eksemplars omfang, der ikke fremgår af omfangsangivelsen."@da ;
        rdakit:toolkitLabel       "note om omfang af eksemplar"@da ;
        rdakit:toolkitDefinition  "Note, der giver oplysninger om det specifikke eksemplars omfang, der ikke fremgår af omfangsangivelsen."@da ;
        rdfs:label                "hat Anmerkung zum Umfang des Exemplars"@de ;
        skos:definition           "Setzt ein Exemplar mit einer Anmerkung, die Informationen über den Umfang eines spezifischen Exemplars liefert, das beschrieben wird, die nicht als Teil des Elements Umfang erfasst werden, in Beziehung."@de ;
        rdakit:toolkitLabel       "Anmerkung zum Umfang des Exemplars"@de ;
        rdakit:toolkitDefinition  "Eine Anmerkung, die Informationen über den Umfang eines spezifischen Exemplars liefert, das beschrieben wird, die nicht als Teil des Elements Umfang erfasst werden."@de ;
        reg:name                  "σημείωσηΣτηνΈκτασηΤουΑντιτύπου"@el ;
        rdfs:label                "έχει σημείωση στην έκταση του αντιτύπου"@el ;
        reg:lexicalAlias          <http://rdaregistry.info/Elements/i/σημείωσηΣτηνΈκτασηΤουΑντιτύπου.el> ;
        skos:definition           "Συνδέει ένα αντίτυπο με μια σημείωση που παρέχει πληροφορίες αναφορικά με την έκταση ενός συγκεκριμένου περιγραφόμενου αντιτύπου η οποία δεν καταχωρίζεται ως μέρος του στοιχείου της έκτασης."@el ;
        rdakit:toolkitLabel       "σημείωση στην έκταση του αντιτύπου"@el ;
        rdakit:toolkitDefinition  "Μια σημείωση που παρέχει πληροφορίες αναφορικά με την έκταση ενός συγκεκριμένου περιγραφόμενου αντιτύπου η οποία δεν καταχωρίζεται ως μέρος του στοιχείου της έκτασης."@el ;
        rdfs:label                "té com a nota sobre extensió d’un ítem"@ca ;
        skos:definition           "Relaciona un item amb una nota que proporciona la informació sobre l’extensió d’un ítem concret que es descriu i que no s’ha enregistrat com a part de l’element Extensió."@ca ;
        rdakit:toolkitLabel       "nota sobre extensió d’un ítem"@ca ;
        rdakit:toolkitDefinition  "Nota que proporciona la informació sobre l’extensió d’un ítem concret que es descriu i que no s’ha enregistrat com a part de l’element Extensió."@ca ;
        reg:name                  "huomautusKappaleenLaajuudesta"@fi ;
        rdfs:label                "huomautus kappaleen laajuudesta"@fi ;
        reg:lexicalAlias          <rdaa:huomautusKappaleenLaajuudesta.fi> ;
        skos:definition           "Liittää kappaleen huomautukseen kuvailun kohteena olevan yksittäisen kappaleen laajuudesta, jota ei merkitä osana varsinaista laajuuselementtiä."@fi ;
        rdakit:toolkitLabel       "huomautus kappaleen laajuudesta"@fi ;
        rdakit:toolkitDefinition  "Huomautus kuvailun kohteen olevan yksittäisen kappaleen laajuudesta, jota ei merkitä osana varsinaista laajuuselementtiä."@fi ;
        reg:name                  "noteSurLimportanceMatérielleDunItem"@fr ;
        reg:lexicalAlias          <http://rdaregistry.info/Elements/i/noteSurLétendueDunItem.fr> ;
        rdakit:toolkitLabel       "note om eksemplarets omfang"@no ;
        rdakit:toolkitDefinition  "En note som gir informasjon om omfanget til et bestemt eksemplar som beskrives, som ikke er registrert som en del av et omfangselement."@no ;
        rdakit:hasElementType     "6" ;
        reg:name                  "megjegyzésPéldányTerjedelméről"@hu ;
        rdfs:label                "van megjegyzése példány terjedelméről"@hu ;
        skos:definition           "Egy példányt hozzákapcsol egy megjegyzéshez, amely egy éppen leírt sajátos példány terjedelméről nyújt információkat, amelyek nincsenek a terjedelem elem részeként rögzítve."@hu ;
        rdakit:toolkitLabel       "megjegyzés példányterjedelemről"@hu ;
        rdakit:toolkitDefinition  "Megjegyzés, amely egy éppen leírt különleges példány terjedelméről szolgáltat információkat, amelyek nincsenek rögzítve a terjedelem elem részeként."@hu .

<http://rdaregistry.info/Elements/i/P40028>
        rdfs:isDefinedBy          <http://rdaregistry.info/Elements/i/> ;
        reg:status                <http://metadataregistry.org/uri/RegStatus/1001> ;
        reg:name                  "noteOnItem"@en ;
        rdfs:label                "has note on item"@en ;
        skos:definition           "Relates an item to a broad unstructured description of one or more attributes of an item."@en ;
        rdf:type                  rdf:Property ;
        rdfs:domain               <http://rdaregistry.info/Elements/c/C10003> ;
        reg:lexicalAlias          <http://rdaregistry.info/Elements/i/noteOnItem.en> ;
        reg:hasUnconstrained      <http://rdaregistry.info/Elements/u/P60470> ;
        rdakit:instructionNumber  "2.21" ;
        rdakit:toolkitLabel       "note on item"@en ;
        rdakit:toolkitDefinition  "A broad unstructured description of one or more attributes of an item."@en ;
        rdfs:label                "a pour note sur un item"@fr ;
        skos:definition           "Met un item en relation avec une description non structurée générale d’un ou plusieurs attributs d’un item."@fr ;
        rdakit:toolkitLabel       "note sur un item"@fr ;
        rdakit:toolkitDefinition  "Description non structurée générale d’un ou plusieurs attributs d’un item."@fr ;
        rdakit:toolkitLabel       "nota sobre el ítem"@es ;
        rdakit:toolkitDefinition  "Una nota que proporciona información sobre los atributos del ítem."@es ;
        reg:hasSubproperty        <http://rdaregistry.info/Elements/i/object/P40028> ;
        rdfs:label                "har anmärkning om exemplaret"@sv ;
        rdakit:toolkitLabel       "anmärkning om exemplaret"@sv ;
        reg:name                  "ghiChúVềBản"@vi ;
        rdfs:label                "có ghi chú về bản"@vi ;
        skos:definition           "Liên kết bản với ghi chú cung cấp thông tin về các thuộc tính của bản."@vi ;
        rdakit:toolkitLabel       "ghi chú về bản"@vi ;
        rdakit:toolkitDefinition  "Ghi chú cung cấp thông tin về các thuộc tính của bản."@vi ;
        reg:name                  "noteOmEksemplar"@da ;
        rdfs:label                "har note om eksemplar"@da ;
        reg:lexicalAlias          <http://rdaregistry.info/Elements/i/noteOmEksemplar.da> ;
        skos:definition           "Relaterer et eksemplar til en note, der giver oplysninger om et eksemplars attributter."@da ;
        rdakit:toolkitLabel       "note om eksemplar"@da ;
        rdakit:toolkitDefinition  "Note, der giver oplysninger om et eksemplars attributter."@da ;
        rdfs:label                "hat Anmerkung zum Exemplar"@de ;
        skos:definition           "Setzt ein Exemplar mit einer Anmerkung, die Informationen über Merkmale eines Exemplars liefert, in Beziehung."@de ;
        rdakit:toolkitLabel       "Anmerkung zum Exemplar"@de ;
        rdakit:toolkitDefinition  "Eine Anmerkung, die Informationen über Merkmale eines Exemplars liefert."@de ;
        reg:name                  "σημείωσηΣτοΑντίτυπο"@el ;
        rdfs:label                "έχει σημείωση στο αντίτυπο"@el ;
        reg:lexicalAlias          <http://rdaregistry.info/Elements/i/σημείωσηΣτοΑντίτυπο.el> ;
        skos:definition           "Συνδέει ένα αντίτυπο με μια σημείωση που παρέχει πληροφορίες σχετικά με τις ιδιότητες ενός αντιτύπου."@el ;
        rdakit:toolkitLabel       "σημείωση στο αντίτυπο"@el ;
        rdakit:toolkitDefinition  "Μια σημείωση που παρέχει πληροφορίες σχετικά με τις ιδιότητες ενός αντιτύπου."@el ;
        rdfs:label                "té com a nota sobre un ítem"@ca ;
        skos:definition           "Relaciona un item amb una nota que proporciona la informació sobre els atributs d’un ítem."@ca ;
        rdakit:toolkitLabel       "nota sobre un ítem"@ca ;
        rdakit:toolkitDefinition  "Nota que proporciona la informació sobre els atributs d’un ítem."@ca ;
        reg:name                  "huomautusKappaleesta"@fi ;
        rdfs:label                "huomautus kappaleesta"@fi ;
        reg:lexicalAlias          <rdaa:huomautusKappaleesta.fi> ;
        skos:definition           "Liittää kappaleen huomautukseen kappaleen attribuutteihin liittyvästä lisätiedosta."@fi ;
        rdakit:toolkitLabel       "huomautus kappaleesta"@fi ;
        rdakit:toolkitDefinition  "Huomautus kappaleen attribuutteihin liittyvistä lisätiedoista."@fi ;
        reg:name                  "noteSurUnItem"@fr ;
        reg:lexicalAlias          <http://rdaregistry.info/Elements/i/noteSurUnItem.fr> ;
        rdakit:toolkitLabel       "note om eksemplar"@no ;
        rdakit:toolkitDefinition  "En note som gir informasjon om attributter for et eksemplar."@no ;
        rdakit:hasElementType     "6" ;
        rdfs:subPropertyOf        <http://rdaregistry.info/Elements/x/P00015> ;
        reg:name                  "megjegyzésPéldányról"@hu ;
        rdfs:label                "van megjegyzése a példányról"@hu ;
        skos:definition           "Egy példányt hozzákapcsol egy megjegyzéshez, amely egy példány ismérveiről nyújt információkat."@hu ;
        rdakit:toolkitLabel       "megjegyzés a példányról"@hu ;
        rdakit:toolkitDefinition  "Megjegyzés, amely információkat nyújt egy példány ismérveiről."@hu ;
        reg:hasSubproperty        <http://rdaregistry.info/Elements/i/datatype/P40028> ;
        reg:hasSubproperty        <http://rdaregistry.info/Elements/i/P40003> .

<http://rdaregistry.info/Elements/i/P40035>
        rdfs:isDefinedBy          <http://rdaregistry.info/Elements/i/> ;
        reg:status                <http://metadataregistry.org/uri/RegStatus/1001> ;
        reg:name                  "onDiscWithItem"@en ;
        rdfs:label                "is on disc with item"@en ;
        skos:definition           "Relates an item to an item that is contained on the same disc as an item."@en ;
        rdf:type                  rdf:Property ;
        rdfs:domain               <http://rdaregistry.info/Elements/c/C10003> ;
        rdfs:subPropertyOf        <http://rdaregistry.info/Elements/i/P40029> ;
        reg:lexicalAlias          <http://rdaregistry.info/Elements/i/onDiscWithItem.en> ;
        reg:hasUnconstrained      <http://rdaregistry.info/Elements/u/P60257> ;
        rdakit:toolkitLabel       "on disc with item"@en ;
        rdakit:toolkitDefinition  "An item that is contained on the same disc as an item."@en ;
        rdfs:label                "est sur le disque avec un item"@fr ;
        skos:definition           "Met un item en relation avec un item qui est contenu sur le même disque qu’un item."@fr ;
        rdakit:toolkitLabel       "sur le disque avec un item"@fr ;
        rdakit:toolkitDefinition  "Item qui est contenu sur le même disque qu’un item."@fr ;
        rdakit:toolkitLabel       "en disco con (ítem)"@es ;
        rdakit:toolkitDefinition  "Un ítem que se incluye en el mismo disco que el ítem descrito."@es ;
        rdakit:instructionNumber  "24.5" ;
        reg:hasSubproperty        <http://rdaregistry.info/Elements/i/object/P40035> ;
        reg:name                  "trênĐĩaVớiBản"@vi ;
        rdfs:label                "là trên đĩa với (bản)"@vi ;
        skos:definition           "Liên kết bản với bản được chứa trên cùng đĩa với bản đang được mô tả"@vi ;
        rdakit:toolkitLabel       "trên đĩa với (bản)"@vi ;
        rdakit:toolkitDefinition  "Bản được chứa trên cùng đĩa với bản đang được mô tả"@vi ;
        reg:name                  "påDiscSammenMedEksemplar"@da ;
        rdfs:label                "er på disc sammen med (eksemplar)"@da ;
        reg:lexicalAlias          <http://rdaregistry.info/Elements/i/påDiscSammenMedEksemplar.da> ;
        skos:definition           "Relaterer et eksemplar til et eksemplar, der er indeholdt på den samme disc som det eksemplar, der beskrives."@da ;
        rdakit:toolkitLabel       "på disc sammen med (eksemplar)"@da ;
        rdakit:toolkitDefinition  "Eksemplar, der er indeholdt på den samme disc som det eksemplar, der beskrives."@da ;
        rdfs:label                "ist auf Disk mit (Exemplar)"@de ;
        skos:definition           "Setzt ein Exemplar mit einem Exemplar, das auf derselben Disk enthalten ist, wie ein Exemplar, das beschrieben wird, in Beziehung."@de ;
        rdakit:toolkitLabel       "Auf Disk mit (Exemplar)"@de ;
        rdakit:toolkitDefinition  "Ein Exemplar, das auf derselben Disk enthalten ist, wie ein Exemplar, das beschrieben wird."@de ;
        reg:name                  "στονΔίσκοΜαζίΜεΑντίτυπο"@el ;
        rdfs:label                "είναι στον δίσκο μαζί με (αντίτυπο)"@el ;
        reg:lexicalAlias          <http://rdaregistry.info/Elements/i/στονΔίσκοΜαζίΜεΑντίτυπο.el> ;
        skos:definition           "Συνδέει ένα αντίτυπο με ένα αντίτυπο το οποίο περιέχεται στον ίδιο δίσκο με ένα περιγραφόμενο αντίτυπο."@el ;
        rdakit:toolkitLabel       "στον δίσκο μαζί με (αντίτυπο)"@el ;
        rdakit:toolkitDefinition  "Ένα αντίτυπο το οποίο περιέχεται στον ίδιο δίσκο με ένα περιγραφόμενο αντίτυπο."@el ;
        rdfs:label                "és en un disc amb (ítem)"@ca ;
        skos:definition           "Relaciona un item amb un ítem inclòs en el mateix disc amb un ítem que es descriu."@ca ;
        rdakit:toolkitLabel       "en un disc amb (ítem)"@ca ;
        rdakit:toolkitDefinition  "Ítem inclòs en el mateix disc amb un ítem que es descriu."@ca ;
        reg:name                  "levyllaMyosKappale"@fi ;
        rdfs:label                "levyllä myös (kappale)"@fi ;
        reg:lexicalAlias          <rdaa:levyllaMyosKappale.fi> ;
        skos:definition           "Liittää kappaleen kappaleeseen, joka on samalla levyllä kuin kuvailun kohde."@fi ;
        rdakit:toolkitLabel       "levyllä myös (kappale)"@fi ;
        rdakit:toolkitDefinition  "Kappale, joka on samalla levyllä kuin kuvailtava kappale."@fi ;
        reg:name                  "surLeDisqueAvecItem"@fr ;
        reg:lexicalAlias          <http://rdaregistry.info/Elements/i/surLeDisqueAvecUnItem.fr> ;
        rdakit:toolkitLabel       "på plate med (eksemplar)"@no ;
        rdakit:toolkitDefinition  "Et eksemplar som befinner seg på samme plate som eksemplaret som beskrives."@no ;
        rdakit:hasElementType     "2" ;
        reg:name                  "egyLemezenPéldánnyal"@hu ;
        rdfs:label                "lemezen (példány)"@hu ;
        skos:definition           "Egy példányt hozzákapcsol egy olyan példányhoz, amelyet ugyanaz a lemez tartalmaz, mint az éppen leírt példányt. "@hu ;
        rdakit:toolkitLabel       "egy lemezen (példány)"@hu ;
        rdakit:toolkitDefinition  "Egy példány, amely egy éppen leírt példánnyal közös lemezen van."@hu .

<http://rdaregistry.info/Elements/i/P40021>
        rdfs:isDefinedBy          <http://rdaregistry.info/Elements/i/> ;
        reg:status                <http://metadataregistry.org/uri/RegStatus/1001> ;
        reg:name                  "ownerAgent"@en ;
        rdfs:label                "has owner agent"@en ;
        skos:definition           "Relates an item to an agent who has current or former legal possession of an item."@en ;
        rdf:type                  rdf:Property ;
        rdfs:domain               <http://rdaregistry.info/Elements/c/C10003> ;
        reg:hasSubproperty        <http://rdaregistry.info/Elements/i/P40018> ;
        reg:hasSubproperty        <http://rdaregistry.info/Elements/i/P40019> ;
        reg:lexicalAlias          <http://rdaregistry.info/Elements/i/ownerAgent.en> ;
        reg:hasUnconstrained      <http://rdaregistry.info/Elements/u/P60404> ;
        rdakit:instructionNumber  "22.2" ;
        rdakit:toolkitLabel       "owner agent"@en ;
        rdakit:toolkitDefinition  "An agent who has current or former legal possession of an item."@en ;
        rdfs:label                "a pour agent propriétaire"@fr ;
        skos:definition           "Met un item en relation avec un agent qui possède actuellement ou a auparavant possédé légalement un item."@fr ;
        rdakit:toolkitLabel       "agent propriétaire"@fr ;
        rdakit:toolkitDefinition  "Agent qui possède actuellement ou a auparavant possédé légalement un item."@fr ;
        rdakit:toolkitLabel       "propietario"@es ;
        rdakit:toolkitDefinition  "Una persona, familia o entidad corporativa que detenta la posesión legal de un ítem (es decir, una copia específica o una instancia de un recurso)."@es ;
        rdfs:label                "har ägare"@sv ;
        rdakit:toolkitLabel       "ägare"@sv ;
        reg:hasSubproperty        <http://rdaregistry.info/Elements/i/object/P40021> ;
        rdfs:subPropertyOf        <http://rdaregistry.info/Elements/i/P40072> ;
        reg:name                  "ngườiChủ"@vi ;
        rdfs:label                "có người chủ"@vi ;
        skos:definition           "Liên kết bản với tác nhân sở hữu theo pháp luật một bản."@vi ;
        rdakit:toolkitLabel       "người chủ"@vi ;
        rdakit:toolkitDefinition  "Tác nhân sở hữu theo pháp luật một bản."@vi ;
        reg:name                  "ejer"@da ;
        rdfs:label                "har ejer"@da ;
        reg:lexicalAlias          <http://rdaregistry.info/Elements/i/ejer.da> ;
        skos:definition           "Relaterer et eksemplar til en agent, der er i lovlig besiddelse af et eksemplar."@da ;
        rdakit:toolkitLabel       "ejer"@da ;
        rdakit:toolkitDefinition  "Agent, der er i lovlig besiddelse af et eksemplar."@da ;
        rdfs:label                "hat Eigentümer"@de ;
        skos:definition           "Setzt ein Exemplar mit einem Akteur, der im rechtmäßigen Besitz eines Exemplars ist, in Beziehung."@de ;
        rdakit:toolkitLabel       "Eigentümer"@de ;
        rdakit:toolkitDefinition  "Ein Akteur, der im rechtmäßigen Besitz eines Exemplars ist."@de ;
        reg:name                  "ιδιοκτήτης"@el ;
        rdfs:label                "έχει ιδιοκτήτη"@el ;
        reg:lexicalAlias          <http://rdaregistry.info/Elements/i/ιδιοκτήτης.el> ;
        skos:definition           "Συνδέει ένα αντίτυπο με έναν φορέα που έχει τη νόμιμη κατοχή ενός αντιτύπου."@el ;
        rdakit:toolkitLabel       "ιδιοκτήτης"@el ;
        rdakit:toolkitDefinition  "Ένας φορέας που έχει τη νόμιμη κατοχή ενός αντιτύπου."@el ;
        rdfs:label                "té com a propietari"@ca ;
        skos:definition           "Relaciona un item amb un agent que posseeix legalment un ítem."@ca ;
        rdakit:toolkitLabel       "propietari"@ca ;
        rdakit:toolkitDefinition  "Agent que posseeix legalment un ítem."@ca ;
        reg:name                  "omistaja"@fi ;
        rdfs:label                "omistaja"@fi ;
        reg:lexicalAlias          <rdaa:omistaja.fi> ;
        skos:definition           "Liittää kappaleen toimijaan, jolla on kappaleen laillinen omistusoikeus."@fi ;
        rdakit:toolkitLabel       "omistaja"@fi ;
        rdakit:toolkitDefinition  "Toimija, jolla on kappaleen laillinen omistusoikeus."@fi ;
        reg:name                  "propriétaire"@fr ;
        reg:lexicalAlias          <http://rdaregistry.info/Elements/i/agentPropriétaire.fr> ;
        rdakit:toolkitLabel       "eier"@no ;
        rdakit:toolkitDefinition  "En agent som er den rettmessige eieren av et eksemplar."@no ;
        rdakit:hasElementType     "2" ;
        reg:name                  "tulajdonos"@hu ;
        rdfs:label                "van tulajdonosa"@hu ;
        skos:definition           "Egy példányt hozzákapcsol egy ágenshez (személyhez, családhoz vagy testülethez), akinek/amelynek jogszerű tulajdonában van egy példány."@hu ;
        rdakit:toolkitLabel       "tulajdonos"@hu ;
        rdakit:toolkitDefinition  "Egy ágens (személy, család vagy testület), akinek/amelynek jogos tulajdonában van egy példány."@hu ;
        skos:altLabel             "owner"@en ;
        reg:hasSubproperty        <http://rdaregistry.info/Elements/i/P40101> ;
        reg:hasSubproperty        <http://rdaregistry.info/Elements/i/P40102> ;
        reg:hasSubproperty        <http://rdaregistry.info/Elements/i/P40117> ;
        reg:hasSubproperty        <http://rdaregistry.info/Elements/i/P40118> ;
        skos:altLabel             "propriétaire"@fr .

<http://rdaregistry.info/Elements/i/P40120>
        rdfs:isDefinedBy          <http://rdaregistry.info/Elements/i/> ;
        reg:status                <http://metadataregistry.org/uri/RegStatus/1001> ;
        rdfs:label                "has owner collective agent"@en ;
        reg:lexicalAlias          <http://rdaregistry.info/Elements/i/ownerCollectiveAgent.en> ;
        skos:definition           "Relates an item to a collective agent who has current or former legal possession of an item."@en ;
        rdakit:toolkitLabel       "owner collective agent"@en ;
        rdakit:toolkitDefinition  "A collective agent who has current or former legal possession of an item."@en ;
        rdf:type                  rdf:Property ;
        reg:name                  "ownerCollectiveAgent" ;
        rdfs:domain               <http://rdaregistry.info/Elements/c/C10003> ;
        rdakit:hasElementType     "2" ;
        reg:hasSubproperty        <http://rdaregistry.info/Elements/i/datatype/P40120> ;
        reg:hasSubproperty        <http://rdaregistry.info/Elements/i/object/P40120> ;
        reg:hasSubproperty        <http://rdaregistry.info/Elements/i/P40117> ;
        reg:hasSubproperty        <http://rdaregistry.info/Elements/i/P40118> ;
        rdfs:subPropertyOf        <http://rdaregistry.info/Elements/i/P40076> ;
        rdfs:subPropertyOf        <http://rdaregistry.info/Elements/i/P40021> ;
        reg:hasSubproperty        <http://rdaregistry.info/Elements/i/P40136> ;
        reg:hasSubproperty        <http://rdaregistry.info/Elements/i/P40152> ;
        reg:hasUnconstrained      <http://rdaregistry.info/Elements/u/P60404> ;
        rdfs:label                "a pour agent collectif propriétaire"@fr ;
        skos:definition           "Met un item en relation avec un agent collectif qui possède actuellement ou a auparavant possédé légalement un item."@fr ;
        rdakit:toolkitLabel       "agent collectif propriétaire"@fr ;
        rdakit:toolkitDefinition  "Agent collectif qui possède actuellement ou a auparavant possédé légalement un item."@fr ;
        reg:lexicalAlias          <http://rdaregistry.info/Elements/i/agentCollectifPropriétaire.fr> .

<http://rdaregistry.info/Elements/i/P40136>
        rdfs:isDefinedBy          <http://rdaregistry.info/Elements/i/> ;
        reg:status                <http://metadataregistry.org/uri/RegStatus/1001> ;
        rdfs:label                "has owner corporate body"@en ;
        reg:lexicalAlias          <http://rdaregistry.info/Elements/i/ownerCorporateBody.en> ;
        skos:definition           "Relates an item to a corporate body who has current or former legal possession of an item."@en ;
        rdakit:toolkitLabel       "owner corporate body"@en ;
        rdakit:toolkitDefinition  "A corporate body who has current or former legal possession of an item."@en ;
        rdf:type                  rdf:Property ;
        reg:name                  "ownerCorporateBody" ;
        rdfs:domain               <http://rdaregistry.info/Elements/c/C10003> ;
        rdakit:hasElementType     "2" ;
        reg:hasSubproperty        <http://rdaregistry.info/Elements/i/datatype/P40136> ;
        reg:hasSubproperty        <http://rdaregistry.info/Elements/i/object/P40136> ;
        reg:hasSubproperty        <http://rdaregistry.info/Elements/i/P40133> ;
        reg:hasSubproperty        <http://rdaregistry.info/Elements/i/P40134> ;
        rdfs:subPropertyOf        <http://rdaregistry.info/Elements/i/P40075> ;
        rdfs:subPropertyOf        <http://rdaregistry.info/Elements/i/P40120> ;
        reg:hasUnconstrained      <http://rdaregistry.info/Elements/u/P60404> ;
        rdfs:label                "a pour collectivité propriétaire"@fr ;
        skos:definition           "Met un item en relation avec une collectivité qui possède actuellement ou a auparavant possédé légalement un item."@fr ;
        rdakit:toolkitLabel       "collectivité propriétaire"@fr ;
        rdakit:toolkitDefinition  "Collectivité qui possède actuellement ou a auparavant possédé légalement un item."@fr ;
        reg:lexicalAlias          <http://rdaregistry.info/Elements/i/collectivitéPropriétaire.fr> .

<http://rdaregistry.info/Elements/i/P40152>
        rdfs:isDefinedBy          <http://rdaregistry.info/Elements/i/> ;
        reg:status                <http://metadataregistry.org/uri/RegStatus/1001> ;
        rdfs:label                "has owner family"@en ;
        reg:lexicalAlias          <http://rdaregistry.info/Elements/i/ownerFamily.en> ;
        skos:definition           "Relates an item to a family who has current or former legal possession of an item."@en ;
        rdakit:toolkitLabel       "owner family"@en ;
        rdakit:toolkitDefinition  "A family who has current or former legal possession of an item."@en ;
        rdf:type                  rdf:Property ;
        reg:name                  "ownerFamily" ;
        rdfs:domain               <http://rdaregistry.info/Elements/c/C10003> ;
        rdakit:hasElementType     "2" ;
        reg:hasSubproperty        <http://rdaregistry.info/Elements/i/datatype/P40152> ;
        reg:hasSubproperty        <http://rdaregistry.info/Elements/i/object/P40152> ;
        reg:hasSubproperty        <http://rdaregistry.info/Elements/i/P40149> ;
        reg:hasSubproperty        <http://rdaregistry.info/Elements/i/P40150> ;
        rdfs:subPropertyOf        <http://rdaregistry.info/Elements/i/P40074> ;
        rdfs:subPropertyOf        <http://rdaregistry.info/Elements/i/P40120> ;
        reg:hasUnconstrained      <http://rdaregistry.info/Elements/u/P60404> ;
        rdfs:label                "a pour famille propriétaire"@fr ;
        skos:definition           "Met un item en relation avec une famille qui possède actuellement ou a auparavant possédé légalement un item."@fr ;
        rdakit:toolkitLabel       "famille propriétaire"@fr ;
        rdakit:toolkitDefinition  "Famille qui possède actuellement ou a auparavant possédé légalement un item."@fr ;
        reg:lexicalAlias          <http://rdaregistry.info/Elements/i/famillePropriétaire.fr> .

<http://rdaregistry.info/Elements/i/P40104>
        rdfs:isDefinedBy          <http://rdaregistry.info/Elements/i/> ;
        reg:status                <http://metadataregistry.org/uri/RegStatus/1001> ;
        rdfs:label                "has owner person"@en ;
        reg:lexicalAlias          <http://rdaregistry.info/Elements/i/ownerPerson.en> ;
        skos:definition           "Relates an item to a person who has current or former legal possession of an item."@en ;
        rdakit:toolkitLabel       "owner person"@en ;
        rdakit:toolkitDefinition  "A person who has current or former legal possession of an item."@en ;
        rdf:type                  rdf:Property ;
        reg:name                  "ownerPerson" ;
        rdfs:domain               <http://rdaregistry.info/Elements/c/C10003> ;
        rdakit:hasElementType     "2" ;
        reg:hasSubproperty        <http://rdaregistry.info/Elements/i/datatype/P40104> ;
        reg:hasSubproperty        <http://rdaregistry.info/Elements/i/object/P40104> ;
        reg:hasSubproperty        <http://rdaregistry.info/Elements/i/P40101> ;
        reg:hasSubproperty        <http://rdaregistry.info/Elements/i/P40102> ;
        rdfs:subPropertyOf        <http://rdaregistry.info/Elements/i/P40073> ;
        rdfs:subPropertyOf        <http://rdaregistry.info/Elements/i/P40021> ;
        reg:hasUnconstrained      <http://rdaregistry.info/Elements/u/P60404> ;
        rdfs:label                "a pour personne propriétaire"@fr ;
        skos:definition           "Met un item en relation avec une personne qui possède actuellement ou a auparavant possédé légalement un item."@fr ;
        rdakit:toolkitLabel       "personne propriétaire"@fr ;
        rdakit:toolkitDefinition  "Personne qui possède actuellement ou a auparavant possédé légalement un item."@fr ;
        reg:lexicalAlias          <http://rdaregistry.info/Elements/i/personnePropriétaire.fr> .

<http://rdaregistry.info/Elements/i/P40085>
        rdfs:isDefinedBy          <http://rdaregistry.info/Elements/i/> ;
        reg:status                <http://metadataregistry.org/uri/RegStatus/1001> ;
        rdf:type                  rdf:Property ;
        reg:name                  "preferredTitleOfItem"@en ;
        rdfs:label                "has preferred title of item"@en ;
        reg:lexicalAlias          <http://rdaregistry.info/Elements/i/preferredTitleOfItem.en> ;
        skos:definition           "Relates an item to a title of item that is selected for preference in a specific application or context."@en ;
        rdfs:domain               <http://rdaregistry.info/Elements/c/C10003> ;
        rdakit:toolkitLabel       "preferred title of item"@en ;
        rdakit:toolkitDefinition  "A title of item that is selected for preference in a specific application or context."@en ;
        rdfs:subPropertyOf        <http://rdaregistry.info/Elements/i/P40082> ;
        reg:hasUnconstrained      <http://rdaregistry.info/Elements/u/P60588> ;
        reg:hasSubproperty        <http://rdaregistry.info/Elements/i/object/P40085> ;
        rdakit:hasElementType     "3" ;
        reg:hasSubproperty        <http://rdaregistry.info/Elements/i/datatype/P40085> ;
        rdfs:subPropertyOf        <http://rdaregistry.info/Elements/x/P00021> ;
        rdfs:label                "a pour titre privilégié d’une œuvre"@fr ;
        skos:definition           "Met un item en relation avec un titre d’item qui fait l’objet d’un choix privilégié dans une application ou un contexte spécifiques."@fr ;
        rdakit:toolkitLabel       "titre privilégié d’une œuvre"@fr ;
        rdakit:toolkitDefinition  "Titre d’item qui fait l’objet d’un choix privilégié dans une application ou un contexte spécifiques."@fr ;
        reg:lexicalAlias          <http://rdaregistry.info/Elements/i/titrePrivilégiéDuneŒuvre.fr> .

<http://rdaregistry.info/Elements/i/P40059>
        rdfs:isDefinedBy          <http://rdaregistry.info/Elements/i/> ;
        reg:status                <http://metadataregistry.org/uri/RegStatus/1008> ;
        rdf:type                  rdf:Property ;
        rdfs:domain               <http://rdaregistry.info/Elements/c/C10003> ;
        reg:hasUnconstrained      <http://rdaregistry.info/Elements/u/P60179> ;
        rdfs:label                "a pour fac-similé de conservation (item)"@fr ;
        skos:definition           "Met un item en relation avec un item qui consiste en une reproduction exacte sur un support de qualité conservation, tel qu’un papier permanent sans acide ou un papier d’archivage."@fr ;
        rdakit:toolkitLabel       "fac-similé de conservation (item)"@fr ;
        rdakit:toolkitDefinition  "Item qui consiste en une reproduction exacte sur un support de qualité conservation, tel qu’un papier permanent sans acide ou un papier d’archivage."@fr ;
        rdakit:toolkitLabel       "facsímil de preservación (ítem)"@es ;
        rdakit:toolkitDefinition  "Un ítem que consiste en una reproducción exacta sobre un medio con calidad de preservación, tal como papel libre de ácido o papel de archivo."@es ;
        rdfs:subPropertyOf        <http://rdaregistry.info/Elements/i/P40058> ;
        rdakit:instructionNumber  "24.5" ;
        reg:hasSubproperty        <http://rdaregistry.info/Elements/i/object/P40059> ;
        reg:name                  "bảoQuảnTrênBảnSaoChép"@vi ;
        rdfs:label                "có sao chép bảo quản (bản)"@vi ;
        skos:definition           "Liên kết bản với bản gồm có bản tạo lại chính xác trên phương tiện chất lượng bảo quản, như là giấy vĩnh cửu phi axit hoặc giấy lưu trữ."@vi ;
        rdakit:toolkitLabel       "bản sao chép bản quản (bản)"@vi ;
        rdakit:toolkitDefinition  "Bản gồm có bản tạo lại chính xác trên phương tiện chất lượng bảo quản, như là giấy vĩnh cửu phi axit hoặc giấy lưu trữ."@vi ;
        reg:name                  "bevaringsfaksimileEksemplar"@da ;
        rdfs:label                "har bevaringsfaksimile (eksemplar)"@da ;
        reg:lexicalAlias          <http://rdaregistry.info/Elements/i/bevaringsfaksimileEksemplar.da> ;
        skos:definition           "Relaterer et eksemplar til et eksemplar, der består af en nøjagtig reproduktion på et medium af bevaringskvalitet, såsom syrefrit permanent- eller arkivpapir."@da ;
        rdakit:toolkitLabel       "bevaringsfaksimile eksemplar"@da ;
        rdakit:toolkitDefinition  "Eksemplar, der består af en nøjagtig reproduktion på et medium af bevaringskvalitet, såsom syrefrit permanent- eller arkivpapir."@da ;
        rdfs:label                "hat Bestandserhaltungsfaksimile (Exemplar)"@de ;
        skos:definition           "Setzt ein Exemplar mit einem Exemplar, das aus einer exakten Reproduktion auf bestandserhaltenden Medien, wie z. B. säurefreiem oder Archivpapier, besteht, in Beziehung."@de ;
        rdakit:toolkitLabel       "Bestandserhaltungsfaksimile (Exemplar)"@de ;
        rdakit:toolkitDefinition  "Ein Exemplar, das aus einer exakten Reproduktion auf bestandserhaltenden Medien, wie z. B. säurefreiem oder Archivpapier, besteht."@de ;
        reg:name                  "διατήρησηOμοιότυπουΑντιτύπου"@el ;
        rdfs:label                "έχει διατήρηση ομοιότυπου (αντίτυπο)"@el ;
        reg:lexicalAlias          <http://rdaregistry.info/Elements/i/διατήρησηOμοιότυπουΑντιτύπου.el> ;
        skos:definition           "Συνδέει ένα αντίτυπο με ένα αντίτυπο το οποίο συνίσταται από μια ακριβή αναπαραγωγή πάνω σε μέσα διατήρησης της ποιότητας, όπως αντιόξινο μόνιμο ή αρχειακό χαρτί."@el ;
        rdakit:toolkitLabel       "διατήρηση ομοιότυπου (αντίτυπο)"@el ;
        rdakit:toolkitDefinition  "Ένα αντίτυπο το οποίο συνίσταται από μια ακριβή αναπαραγωγή πάνω σε μέσα διατήρησης της ποιότητας, όπως αντιόξινο μόνιμο ή αρχειακό χαρτί."@el ;
        rdfs:label                "té com a facsímil de preservació (ítem)"@ca ;
        skos:definition           "Relaciona un item amb un ítem que consisteix en una reproducció exacta en un suport de preservació de qualitat, com ara paper permanent no àcid o paper d’arxiu."@ca ;
        rdakit:toolkitLabel       "facsímil de preservació (ítem)"@ca ;
        rdakit:toolkitDefinition  "Ítem que consisteix en una reproducció exacta en un suport de preservació de qualitat, com ara paper permanent no àcid o paper d’arxiu."@ca ;
        reg:name                  "sailytyskopioKappale"@fi ;
        rdfs:label                "säilytyskopio (kappale)"@fi ;
        reg:lexicalAlias          <rdaa:sailytyskopioKappale.fi> ;
        skos:definition           "Liittää kappaleen kappaleeseen, joka on arkistokelpoinen (kuten hapoton arkistopaperi), täysin identtinen jäljennös."@fi ;
        rdakit:toolkitLabel       "säilytyskopio (kappale)"@fi ;
        rdakit:toolkitDefinition  "Kappale, joka on arkistokelpoinen (kuten hapoton arkistopaperi), täysin identtinen jäljennös."@fi ;
        reg:name                  "facsimiléDeConservationItem"@fr ;
        reg:lexicalAlias          <http://rdaregistry.info/Elements/i/facsimiléDeConservationItem.fr> ;
        rdakit:toolkitLabel       "bevaringskopi (eksemplar)"@no ;
        rdakit:toolkitDefinition  "Et eksemplar som består av en eksakt reproduksjon på et medium av bevaringskvalitet, for eksempel syrefritt pergament eller arkivpapir."@no ;
        reg:hasSubproperty        <http://rdaregistry.info/Elements/i/datatype/P40059> .

<http://rdaregistry.info/Elements/i/P40090>
        rdfs:isDefinedBy          <http://rdaregistry.info/Elements/i/> ;
        reg:status                <http://metadataregistry.org/uri/RegStatus/1001> ;
        rdfs:label                "has preservation facsimile of item"@en ;
        rdf:type                  rdf:Property ;
        reg:name                  "preservationFacsimileOfItem"@en ;
        reg:lexicalAlias          <http://rdaregistry.info/Elements/i/preservationFacsimileOfItem.en> ;
        skos:definition           "Relates an item to a manifestation that consists of an exact reproduction of an item on preservation-quality media, such as acid-free permanent or archival paper."@en ;
        rdfs:domain               <http://rdaregistry.info/Elements/c/C10003> ;
        rdfs:subPropertyOf        <http://rdaregistry.info/Elements/i/P40089> ;
        rdakit:toolkitLabel       "preservation facsimile of item"@en ;
        rdakit:toolkitDefinition  "A manifestation that consists of an exact reproduction of an item on preservation-quality media, such as acid-free permanent or archival paper."@en ;
        reg:hasUnconstrained      <http://rdaregistry.info/Elements/u/P60179> ;
        rdakit:hasElementType     "2" ;
        reg:hasSubproperty        <http://rdaregistry.info/Elements/i/datatype/P40090> ;
        rdfs:label                "a pour fac-similé de conservation d’un item"@fr ;
        skos:definition           "Met un item en relation avec une manifestation qui consiste en une reproduction exacte d’un item sur un support de qualité conservation, tel qu’un papier permanent sans acide ou un papier d’archivage."@fr ;
        rdakit:toolkitLabel       "fac-similé de conservation d’un item"@fr ;
        rdakit:toolkitDefinition  "Manifestation qui consiste en une reproduction exacte d’un item sur un support de qualité conservation, tel qu’un papier permanent sans acide ou un papier d’archivage."@fr ;
        reg:lexicalAlias          <http://rdaregistry.info/Elements/i/facsimiléDeConservationDunItem.fr> ;
        skos:altLabel             "preservation facsimile (item)"@en .

<http://rdaregistry.info/Elements/i/P40044>
        rdfs:isDefinedBy          <http://rdaregistry.info/Elements/i/> ;
        reg:status                <http://metadataregistry.org/uri/RegStatus/1008> ;
        rdf:type                  rdf:Property ;
        rdfs:domain               <http://rdaregistry.info/Elements/c/C10003> ;
        rdfs:subPropertyOf        <http://rdaregistry.info/Elements/i/P40045> ;
        reg:hasUnconstrained      <http://rdaregistry.info/Elements/u/P60299> ;
        rdfs:label                "est un fac-similé de conservation de (item)"@fr ;
        skos:definition           "Met un item en relation avec un item qui sert de base à une reproduction exacte sur un support de qualité conservation, tel qu’un papier permanent sans acide ou un papier d’archivage."@fr ;
        rdakit:toolkitLabel       "fac-similé de conservation de (item)"@fr ;
        rdakit:toolkitDefinition  "Item qui sert de base à une reproduction exacte sur un support de qualité conservation, tel qu’un papier permanent sans acide ou un papier d’archivage."@fr ;
        rdakit:toolkitLabel       "facsímil de preservación de (ítem)"@es ;
        rdakit:toolkitDefinition  "Un ítem utilizado como base para una reproducción exacta sobre un medio con calidad de preservación, tal como papel libre de ácido o papel de archivo."@es ;
        rdakit:instructionNumber  "24.5" ;
        reg:hasSubproperty        <http://rdaregistry.info/Elements/i/object/P40044> ;
        reg:name                  "bảoQuảnTrênBảnSaoCủaBản"@vi ;
        rdfs:label                "là bản sao bảo quản của (bản)"@vi ;
        skos:definition           "Liên kết bản với bản được sử dụng như là cơ sở cho sản xuất lại chính xác trên phương tiện chất lượng bảo quản, như là giấy vĩnh cửu phi axit hoặc giấy lưu trữ."@vi ;
        rdakit:toolkitLabel       "bảo quản trên bản sao của (bản)"@vi ;
        rdakit:toolkitDefinition  "Bản được sử dụng như là cơ sở cho sản xuất lại chính xác trên phương tiện chất lượng bảo quản, như là giấy vĩnh cửu phi axit hoặc giấy lưu trữ."@vi ;
        reg:name                  "bevaringsfaksimileAfEksemplar"@da ;
        rdfs:label                "er bevaringsfaksimile af (eksemplar)"@da ;
        reg:lexicalAlias          <http://rdaregistry.info/Elements/i/bevaringsfaksimileAfEksemplar.da> ;
        skos:definition           "Relaterer et eksemplar til et eksemplar, der er anvendt som grundlag for en nøjagtig reproduktion på et medium af bevaringskvalitet, såsom syrefrit permanent- eller arkivpapir."@da ;
        rdakit:toolkitLabel       "bevaringsfaksimile af eksemplar"@da ;
        rdakit:toolkitDefinition  "Eksemplar, der er anvendt som grundlag for en nøjagtig reproduktion på et medium af bevaringskvalitet, såsom syrefrit permanent- eller arkivpapir."@da ;
        rdfs:label                "ist Bestandserhaltungsfaksimile von (Exemplar)"@de ;
        skos:definition           "Setzt ein Exemplar mit einem Exemplar, das als Grundlage für eine exakte Reproduktion auf bestandserhaltenden Medien, wie z. B. säurefreiem oder Archivpapier, verwendet wurde, in Beziehung."@de ;
        rdakit:toolkitLabel       "Bestandserhaltungsfaksimile von (Exemplar)"@de ;
        rdakit:toolkitDefinition  "Ein Exemplar, das als Grundlage für eine exakte Reproduktion auf bestandserhaltenden Medien, wie z. B. säurefreiem oder Archivpapier, verwendet wurde."@de ;
        reg:name                  "διατήρησηΟμοιότυπουΤουΑντιτύπου"@el ;
        rdfs:label                "είναι διατηρημένο ομοιότυπο του (αντίτυπο)"@el ;
        reg:lexicalAlias          <http://rdaregistry.info/Elements/i/διατήρησηΟμοιότυπουΤουΑντιτύπου.el> ;
        skos:definition           "Συνδέει ένα αντίτυπο με ένα αντίτυπο το οποίο χρησιμοποιείται ως η βάση για μια αναπαραγωγή ακριβείας σε μέσα διατήρησης της ποιότητας, όπως μόνιμο αντιόξινο ή αρχειακό χαρτί."@el ;
        rdakit:toolkitLabel       "διατηρημένο ομοιότυπο του (αντίτυπο)"@el ;
        rdakit:toolkitDefinition  "Ένα αντίτυπο το οποίο χρησιμοποιείται ως η βάση για μια αναπαραγωγή ακριβείας σε μέσα διατήρησης της ποιότητας, όπως μόνιμο αντιόξινο ή αρχειακό χαρτί."@el ;
        rdfs:label                "és facsímil de preservació de (ítem)"@ca ;
        skos:definition           "Relaciona un item amb un ítem que s’usa com a base d’una reproducció exacta en un suport de preservació de qualitat, com ara paper permanent no àcid o paper d’arxiu."@ca ;
        rdakit:toolkitLabel       "facsímil de preservació de (ítem)"@ca ;
        rdakit:toolkitDefinition  "Ítem que s’usa com a base d’una reproducció exacta en un suport de preservació de qualitat, com ara paper permanent no àcid o paper d’arxiu."@ca ;
        reg:name                  "sailytyskopioKappaleesta"@fi ;
        rdfs:label                "säilytyskopio kappaleesta"@fi ;
        reg:lexicalAlias          <rdaa:sailytyskopioKappaleesta.fi> ;
        skos:definition           "Liittää kappaleen kappaleeseen,  jota on käytetty arkistokelpoisen (kuten hapottoman arkistopaperin), täysin identtisen jäljennöksen perustana."@fi ;
        rdakit:toolkitLabel       "säilytyskopio kappaleesta"@fi ;
        rdakit:toolkitDefinition  "Kappale, jota on käytetty arkistokelpoisen (kuten hapottoman arkistopaperin), täysin identtisen jäljennöksen perustana."@fi ;
        reg:name                  "facsimiléDeConservationDeItem"@fr ;
        reg:lexicalAlias          <http://rdaregistry.info/Elements/i/facsimiléDeConservationDeItem.fr> ;
        rdakit:toolkitLabel       "bevaringskopi av (eksemplar)"@no ;
        rdakit:toolkitDefinition  "Et eksemplar som brukes som utgangspunkt for en eksakt reproduksjon på et medium av bevaringskvalitet, for eksempel syrefritt pergament eller arkivpapir."@no ;
        reg:hasSubproperty        <http://rdaregistry.info/Elements/i/datatype/P40044> .

<http://rdaregistry.info/Elements/i/P40072>
        rdfs:isDefinedBy          <http://rdaregistry.info/Elements/i/> ;
        reg:status                <http://metadataregistry.org/uri/RegStatus/1001> ;
        rdfs:subPropertyOf        <http://rdaregistry.info/Elements/i/P40068> ;
        rdf:type                  rdf:Property ;
        reg:name                  "relatedAgentOfItem"@en ;
        rdfs:label                "has related agent of item"@en ;
        reg:lexicalAlias          <http://rdaregistry.info/Elements/i/relatedAgentOfItem.en> ;
        skos:definition           "Relates an item to an agent who is associated with an item."@en ;
        rdfs:domain               <http://rdaregistry.info/Elements/c/C10003> ;
        reg:hasSubproperty        <http://rdaregistry.info/Elements/i/P40073> ;
        reg:hasSubproperty        <http://rdaregistry.info/Elements/i/P40076> ;
        reg:hasSubproperty        <http://rdaregistry.info/Elements/i/datatype/P40072> ;
        reg:hasSubproperty        <http://rdaregistry.info/Elements/i/object/P40072> ;
        reg:name                  "bảnTácNhânCóLiênQuan"@vi ;
        rdfs:label                "có tác nhân có liên quan (bản)"@vi ;
        skos:definition           "Liên kết bản với tác nhân liên quan với bản đang được mô tả."@vi ;
        reg:name                  "relateretAgentEksemplar"@da ;
        rdfs:label                "har relateret agent (eksemplar)"@da ;
        reg:lexicalAlias          <http://rdaregistry.info/Elements/i/relateretAgentEksemplar.da> ;
        skos:definition           "Relaterer et eksemplar til en agent, der er knyttet til et beskrevet eksemplar."@da ;
        reg:name                  "σχετικόςΦορέαςΑντιτύπου"@el ;
        rdfs:label                "έχει σχετικό φορέα (αντίτυπο)"@el ;
        reg:lexicalAlias          <http://rdaregistry.info/Elements/i/σχετικόςΦορέαςΑντιτύπου.el> ;
        skos:definition           "Συνδέει ένα αντίτυπο με έναν φορέα που συνδέεται με ένα περιγραφόμενο αντίτυπο."@el ;
        rdfs:label                "té com a agent relacionat (ítem)"@ca ;
        skos:definition           "Relaciona un item amb un agent associat amb un ítem que es descriu."@ca ;
        reg:name                  "kappaleeseenLiittyvaToimija"@fi ;
        rdfs:label                "kappaleeseen liittyvä toimija"@fi ;
        reg:lexicalAlias          <rdaa:kappaleeseenLiittyvaToimija.fi> ;
        reg:name                  "agentEnRelationItem"@fr ;
        rdfs:label                "a pour agent en relation avec un item"@fr ;
        reg:lexicalAlias          <http://rdaregistry.info/Elements/i/agentEnRelationAvecUnItem.fr> ;
        skos:definition           "Met un item en relation avec un agent qui est associé à un item."@fr ;
        rdakit:toolkitLabel       "related agent of item"@en ;
        rdakit:toolkitDefinition  "An agent who is associated with an item."@en ;
        rdakit:hasElementType     "1" ;
        rdfs:subPropertyOf        <http://rdaregistry.info/Elements/x/P00006> ;
        reg:name                  "kapcsolódóÁgensPéldány"@hu ;
        rdfs:label                "van kapcsolódó ágense (példány)"@hu ;
        skos:definition           "Egy példányt hozzákapcsol egy ágenshez (személyhez, családhoz vagy testülethez), aki/amely egy éppen leírt példányhoz kötődik."@hu ;
        reg:hasUnconstrained      <http://rdaregistry.info/Elements/u/P61008> ;
        reg:hasSubproperty        <http://rdaregistry.info/Elements/i/P40020> ;
        reg:hasSubproperty        <http://rdaregistry.info/Elements/i/P40097> ;
        reg:hasSubproperty        <http://rdaregistry.info/Elements/i/P40098> ;
        reg:hasSubproperty        <http://rdaregistry.info/Elements/i/P40099> ;
        reg:hasSubproperty        <http://rdaregistry.info/Elements/i/P40100> ;
        reg:hasSubproperty        <http://rdaregistry.info/Elements/i/P40103> ;
        reg:hasSubproperty        <http://rdaregistry.info/Elements/i/P40104> ;
        reg:hasSubproperty        <http://rdaregistry.info/Elements/i/P40110> ;
        reg:hasSubproperty        <http://rdaregistry.info/Elements/i/P40111> ;
        reg:hasSubproperty        <http://rdaregistry.info/Elements/i/P40112> ;
        reg:hasSubproperty        <http://rdaregistry.info/Elements/i/P40113> ;
        reg:hasSubproperty        <http://rdaregistry.info/Elements/i/P40114> ;
        reg:hasSubproperty        <http://rdaregistry.info/Elements/i/P40115> ;
        reg:hasSubproperty        <http://rdaregistry.info/Elements/i/P40116> ;
        reg:hasSubproperty        <http://rdaregistry.info/Elements/i/P40119> ;
        reg:hasSubproperty        <http://rdaregistry.info/Elements/i/P40120> ;
        reg:hasSubproperty        <http://rdaregistry.info/Elements/i/P40126> ;
        reg:hasSubproperty        <http://rdaregistry.info/Elements/i/P40127> ;
        reg:hasSubproperty        <http://rdaregistry.info/Elements/i/P40128> ;
        rdakit:toolkitLabel       "agent en relation avec un item"@fr ;
        rdakit:toolkitDefinition  "Agent qui est associé à un item."@fr ;
        skos:altLabel             "other agent associated with item"@en .

<http://rdaregistry.info/Elements/i/P40076>
        rdfs:isDefinedBy          <http://rdaregistry.info/Elements/i/> ;
        reg:status                <http://metadataregistry.org/uri/RegStatus/1001> ;
        rdfs:subPropertyOf        <http://rdaregistry.info/Elements/i/P40072> ;
        rdf:type                  rdf:Property ;
        reg:name                  "relatedCollectiveAgentOfItem"@en ;
        rdfs:label                "has related collective agent of item"@en ;
        reg:lexicalAlias          <http://rdaregistry.info/Elements/i/relatedCollectiveAgentOfItem.en> ;
        skos:definition           "Relates an item to a collective agent who is associated with an item."@en ;
        rdfs:domain               <http://rdaregistry.info/Elements/c/C10003> ;
        reg:hasSubproperty        <http://rdaregistry.info/Elements/i/P40074> ;
        reg:hasSubproperty        <http://rdaregistry.info/Elements/i/P40075> ;
        reg:hasSubproperty        <http://rdaregistry.info/Elements/i/datatype/P40076> ;
        reg:hasSubproperty        <http://rdaregistry.info/Elements/i/object/P40076> ;
        reg:name                  "bảnTácNhânTậpThểCóLiênQuan"@vi ;
        rdfs:label                "có tác nhân tập thể có liên quan (bản)"@vi ;
        skos:definition           "Liên kết bản với tác nhân tập thể liên quan với bản đang được mô tả."@vi ;
        reg:name                  "relaretetKollektivAgent"@da ;
        rdfs:label                "har relateret kollektiv agent (eksemplar)"@da ;
        reg:lexicalAlias          <http://rdaregistry.info/Elements/i/relaretetKollektivAgent.da> ;
        skos:definition           "Relaterer et eksemplar til en kollektiv agent, der er knyttet til et beskrevet eksemplar."@da ;
        reg:name                  "σχετικόςΣυλλογικόςΦορέαςΑντιτύπου"@el ;
        rdfs:label                "έχει σχετικό συλλογικό φορέα (αντίτυπο)"@el ;
        reg:lexicalAlias          <http://rdaregistry.info/Elements/i/σχετικόςΣυλλογικόςΦορέαςΑντιτύπου.el> ;
        skos:definition           "Συνδέει ένα αντίτυπο με έναν συλλογικό φορέα που συνδέεται με ένα περιγραφόμενο αντίτυπο."@el ;
        rdfs:label                "té com a agent col·lectiu relacionat (ítem)"@ca ;
        skos:definition           "Relaciona un item amb un agent col·lectiu associat amb un ítem que es descriu."@ca ;
        reg:name                  "kappaleeseenLiittyvaYhteistoimija"@fi ;
        rdfs:label                "kappaleeseen liittyvä yhteistoimija"@fi ;
        reg:lexicalAlias          <rdaa:kappaleeseenLiittyvaYhteistoimija.fi> ;
        reg:name                  "agentCollectifEnRelationItem"@fr ;
        rdfs:label                "a pour agent collectif en relation avec un item"@fr ;
        reg:lexicalAlias          <http://rdaregistry.info/Elements/i/agentCollectifEnRelationAvecUnItem.fr> ;
        skos:definition           "Met un item en relation avec un agent collectif qui est associé à un item."@fr ;
        rdakit:toolkitLabel       "related collective agent of item"@en ;
        rdakit:toolkitDefinition  "A collective agent who is associated with an item."@en ;
        rdakit:hasElementType     "1" ;
        rdfs:subPropertyOf        <http://rdaregistry.info/Elements/x/P00012> ;
        reg:name                  "kapcsolódóKollektívÁgensPéldány"@hu ;
        rdfs:label                "van kapcsolódó kollektív ágense (példány)"@hu ;
        skos:definition           "Egy példányt hozzákapcsol egy kollektív ágenshez, amely egy éppen leírt példányhoz kötődik."@hu ;
        reg:hasUnconstrained      <http://rdaregistry.info/Elements/u/P61008> ;
        reg:hasSubproperty        <http://rdaregistry.info/Elements/i/P40113> ;
        reg:hasSubproperty        <http://rdaregistry.info/Elements/i/P40114> ;
        reg:hasSubproperty        <http://rdaregistry.info/Elements/i/P40115> ;
        reg:hasSubproperty        <http://rdaregistry.info/Elements/i/P40116> ;
        reg:hasSubproperty        <http://rdaregistry.info/Elements/i/P40119> ;
        reg:hasSubproperty        <http://rdaregistry.info/Elements/i/P40120> ;
        reg:hasSubproperty        <http://rdaregistry.info/Elements/i/P40126> ;
        reg:hasSubproperty        <http://rdaregistry.info/Elements/i/P40127> ;
        reg:hasSubproperty        <http://rdaregistry.info/Elements/i/P40128> ;
        rdakit:toolkitLabel       "agent collectif en relation avec un item"@fr ;
        rdakit:toolkitDefinition  "Agent collectif qui est associé à un item."@fr .

<http://rdaregistry.info/Elements/i/P40075>
        rdfs:isDefinedBy          <http://rdaregistry.info/Elements/i/> ;
        reg:status                <http://metadataregistry.org/uri/RegStatus/1001> ;
        rdfs:subPropertyOf        <http://rdaregistry.info/Elements/i/P40076> ;
        rdf:type                  rdf:Property ;
        reg:name                  "relatedCorporateBodyOfItem"@en ;
        rdfs:label                "has related corporate body of item"@en ;
        reg:lexicalAlias          <http://rdaregistry.info/Elements/i/relatedCorporateBodyOfItem.en> ;
        skos:definition           "Relates an item to a corporate body who is associated with an item."@en ;
        rdfs:domain               <http://rdaregistry.info/Elements/c/C10003> ;
        reg:hasSubproperty        <http://rdaregistry.info/Elements/i/datatype/P40075> ;
        reg:hasSubproperty        <http://rdaregistry.info/Elements/i/object/P40075> ;
        reg:name                  "bảnTậpThểCóLiênQuan"@vi ;
        rdfs:label                "có tập thể có liên quan (bản)"@vi ;
        skos:definition           "Liên kết bản với tập thể liên quan với bản đang được mô tả."@vi ;
        reg:name                  "relateretKorporationEksemplar"@da ;
        rdfs:label                "har relateret korporation (eksemplar)"@da ;
        reg:lexicalAlias          <http://rdaregistry.info/Elements/i/relateretKorporationEksemplar.da> ;
        skos:definition           "Relaterer et eksemplar til en korporation, der er knyttet til et beskrevet eksemplar."@da ;
        reg:name                  "σχετικόΣυλλογικόΌργανοΑντιτύπου"@el ;
        rdfs:label                "έχει σχετικό συλλογικό όργανο (αντίτυπο)"@el ;
        reg:lexicalAlias          <http://rdaregistry.info/Elements/i/σχετικόΣυλλογικόΌργανοΑντιτύπου.el> ;
        skos:definition           "Συνδέει ένα αντίτυπο με ένα συλλογικό όργανο που συνδέεται με ένα περιγραφόμενο αντίτυπο."@el ;
        rdfs:label                "té com a entitat corporativa relacionada (ítem)"@ca ;
        skos:definition           "Relaciona un item amb una entitat corporativa associada amb un ítem que es descriu."@ca ;
        reg:name                  "kappaleeseenLiittyvaYhteiso"@fi ;
        rdfs:label                "kappaleeseen liittyvä yhteisö"@fi ;
        reg:lexicalAlias          <rdaa:kappaleeseenLiittyvaYhteiso.fi> ;
        reg:name                  "collectivitéEnRelationItem"@fr ;
        rdfs:label                "a pour collectivité en relation avec un item"@fr ;
        reg:lexicalAlias          <http://rdaregistry.info/Elements/i/collectivitéEnRelationAvecUnItem.fr> ;
        skos:definition           "Met un item en relation avec une collectivité qui est associée à un item."@fr ;
        rdakit:toolkitLabel       "related corporate body of item"@en ;
        rdakit:toolkitDefinition  "A corporate body who is associated with an item."@en ;
        rdakit:hasElementType     "1" ;
        rdfs:subPropertyOf        <http://rdaregistry.info/Elements/x/P00009> ;
        reg:name                  "kapcsolódóTestületPéldány"@hu ;
        rdfs:label                "van kapcsolódó testülete (példány)"@hu ;
        skos:definition           "Egy példányt hozzákapcsol egy testülethez, amely egy éppen leírt példányhoz kötődik."@hu ;
        reg:hasUnconstrained      <http://rdaregistry.info/Elements/u/P61008> ;
        reg:hasSubproperty        <http://rdaregistry.info/Elements/i/P40129> ;
        reg:hasSubproperty        <http://rdaregistry.info/Elements/i/P40130> ;
        reg:hasSubproperty        <http://rdaregistry.info/Elements/i/P40131> ;
        reg:hasSubproperty        <http://rdaregistry.info/Elements/i/P40132> ;
        reg:hasSubproperty        <http://rdaregistry.info/Elements/i/P40135> ;
        reg:hasSubproperty        <http://rdaregistry.info/Elements/i/P40136> ;
        reg:hasSubproperty        <http://rdaregistry.info/Elements/i/P40142> ;
        reg:hasSubproperty        <http://rdaregistry.info/Elements/i/P40143> ;
        reg:hasSubproperty        <http://rdaregistry.info/Elements/i/P40144> ;
        rdakit:toolkitLabel       "collectivité en relation avec un item"@fr ;
        rdakit:toolkitDefinition  "Collectivité qui est associée à un item."@fr .

<http://rdaregistry.info/Elements/i/P40095>
        rdfs:isDefinedBy          <http://rdaregistry.info/Elements/i/> ;
        reg:status                <http://metadataregistry.org/uri/RegStatus/1001> ;
        rdfs:label                "has related entity of item"@en ;
        reg:lexicalAlias          <http://rdaregistry.info/Elements/i/relatedEntityOfItem.en> ;
        skos:definition           "Relates an item to an entity that is associated with an item."@en ;
        rdakit:toolkitLabel       "related entity of item"@en ;
        rdakit:toolkitDefinition  "An entity that is associated with an item."@en ;
        rdf:type                  rdf:Property ;
        reg:name                  "relatedEntityOfItem" ;
        rdfs:domain               <http://rdaregistry.info/Elements/c/C10003> ;
        rdakit:hasElementType     "1" ;
        rdfs:subPropertyOf        <http://rdaregistry.info/Elements/x/P00028> ;
        reg:hasUnconstrained      <http://rdaregistry.info/Elements/u/P61034> ;
        rdfs:label                "a pour entité en relation avec un item"@fr ;
        skos:definition           "Met un item en relation avec une entité qui est associée à un item."@fr ;
        rdakit:toolkitLabel       "entité en relation avec un item"@fr ;
        rdakit:toolkitDefinition  "Entité qui est associée à un item."@fr ;
        reg:lexicalAlias          <http://rdaregistry.info/Elements/i/entitéEnRelationAvecUnItem.fr> .

<http://rdaregistry.info/Elements/i/P40070>
        rdfs:isDefinedBy          <http://rdaregistry.info/Elements/i/> ;
        reg:status                <http://metadataregistry.org/uri/RegStatus/1001> ;
        rdfs:subPropertyOf        <http://rdaregistry.info/Elements/i/P40068> ;
        rdf:type                  rdf:Property ;
        reg:name                  "relatedExpressionOfItem"@en ;
        rdfs:label                "has related expression of item"@en ;
        reg:lexicalAlias          <http://rdaregistry.info/Elements/i/relatedExpressionOfItem.en> ;
        skos:definition           "Relates an item to an expression that is associated with an item."@en ;
        rdfs:domain               <http://rdaregistry.info/Elements/c/C10003> ;
        reg:hasUnconstrained      <http://rdaregistry.info/Elements/u/P60313> ;
        reg:hasSubproperty        <http://rdaregistry.info/Elements/i/datatype/P40070> ;
        reg:hasSubproperty        <http://rdaregistry.info/Elements/i/object/P40070> ;
        reg:name                  "bảnBiểuHiệnCóLiênQuan"@vi ;
        rdfs:label                "có biểu hiện có liên quan (bản)"@vi ;
        skos:definition           "Liên kết bản với biểu hiện liên quan với bản đang được mô tả."@vi ;
        reg:name                  "relateretUdtrykEksemplar"@da ;
        rdfs:label                "har relateret udtryk (eksemplar)"@da ;
        reg:lexicalAlias          <http://rdaregistry.info/Elements/i/relateretUdtrykEksemplar.da> ;
        skos:definition           "Relaterer et eksemplar til et udtryk, der er knyttet til et beskrevet eksemplar."@da ;
        reg:name                  "σχετικήΈκφρασηΑντιτύπου"@el ;
        rdfs:label                "έχει σχετική έκφραση (αντίτυπο)"@el ;
        reg:lexicalAlias          <http://rdaregistry.info/Elements/i/σχετικήΈκφρασηΑντιτύπου.el> ;
        skos:definition           "Συνδέει ένα αντίτυπο με μια έκφραση συνδεδεμένη με ένα περιγραφόμενο αντίτυπο."@el ;
        rdfs:label                "té com a expressió relacionada (ítem)"@ca ;
        skos:definition           "Relaciona un item amb una expressió associada amb un ítem que es descriu."@ca ;
        reg:name                  "kappaleeseenLiittyvaEkspressio"@fi ;
        rdfs:label                "kappaleeseen liittyvä ekspressio"@fi ;
        reg:lexicalAlias          <rdaa:kappaleeseenLiittyvaEkspressio.fi> ;
        reg:name                  "expressionEnRelationItem"@fr ;
        rdfs:label                "a pour expression en relation avec un item"@fr ;
        reg:lexicalAlias          <http://rdaregistry.info/Elements/i/expressionEnRelationAvecUnItem.fr> ;
        skos:definition           "Met un item en relation avec une expression qui est associée à un item."@fr ;
        rdakit:toolkitLabel       "related expression of item"@en ;
        rdakit:toolkitDefinition  "An expression that is associated with an item."@en ;
        rdakit:hasElementType     "1" ;
        rdfs:subPropertyOf        <http://rdaregistry.info/Elements/x/P00003> ;
        reg:name                  "kapcsolódóKifejezésiformaPéldány"@hu ;
        rdfs:label                "van kapcsolódó kifejezési formája (példány)"@hu ;
        skos:definition           "Egy példányt hozzákapcsol egy olyan kifejezési formához, amely egy éppen leírt példányhoz kötődik."@hu ;
        rdakit:toolkitLabel       "expression en relation avec un item"@fr ;
        rdakit:toolkitDefinition  "Expression qui est associée à un item."@fr .

<http://rdaregistry.info/Elements/i/P40074>
        rdfs:isDefinedBy          <http://rdaregistry.info/Elements/i/> ;
        reg:status                <http://metadataregistry.org/uri/RegStatus/1001> ;
        rdfs:subPropertyOf        <http://rdaregistry.info/Elements/i/P40076> ;
        rdf:type                  rdf:Property ;
        reg:name                  "relatedFamilyOfItem"@en ;
        rdfs:label                "has related family of item"@en ;
        reg:lexicalAlias          <http://rdaregistry.info/Elements/i/relatedFamilyOfItem.en> ;
        skos:definition           "Relates an item to a family who is associated with an item."@en ;
        rdfs:domain               <http://rdaregistry.info/Elements/c/C10003> ;
        reg:hasSubproperty        <http://rdaregistry.info/Elements/i/datatype/P40074> ;
        reg:hasSubproperty        <http://rdaregistry.info/Elements/i/object/P40074> ;
        reg:name                  "bảnGiaĐìnhCóLiênQuan"@vi ;
        rdfs:label                "có gia đình có liên quan (bản)"@vi ;
        skos:definition           "Liên kết bản với gia đình liên quan với bản đang được mô tả."@vi ;
        reg:name                  "relateretFamilieEksemplar"@da ;
        rdfs:label                "har relateret familie (eksemplar)"@da ;
        reg:lexicalAlias          <http://rdaregistry.info/Elements/i/relateretFamilieEksemplar.da> ;
        skos:definition           "Relaterer et eksemplar til en familie, der er knyttet til et beskrevet eksemplar."@da ;
        reg:name                  "σχετικήΟικογένειαΑντιτύπου"@el ;
        rdfs:label                "έχει σχετική οικογένεια (αντίτυπο)"@el ;
        reg:lexicalAlias          <http://rdaregistry.info/Elements/i/σχετικήΟικογένειαΑντιτύπου.el> ;
        skos:definition           "Συνδέει ένα αντίτυπο με μια οικογένεια που συνδέεται με ένα περιγραφόμενο αντίτυπο."@el ;
        rdfs:label                "té com a família relacionada (ítem)"@ca ;
        skos:definition           "Relaciona un item amb una família associada amb un ítem que es descriu."@ca ;
        reg:name                  "kappaleeseenLiittyvaSuku"@fi ;
        rdfs:label                "kappaleeseen liittyvä suku"@fi ;
        reg:lexicalAlias          <rdaa:kappaleeseenLiittyvaSuku.fi> ;
        reg:name                  "familleEnRelationItem"@fr ;
        rdfs:label                "a pour famille en relation avec un item"@fr ;
        reg:lexicalAlias          <http://rdaregistry.info/Elements/i/familleEnRelationAvecUnItem.fr> ;
        skos:definition           "Met un item en relation avec une famille qui est associée à un item."@fr ;
        rdakit:toolkitLabel       "related family of item"@en ;
        rdakit:toolkitDefinition  "A family who is associated with an item."@en ;
        rdakit:hasElementType     "1" ;
        rdfs:subPropertyOf        <http://rdaregistry.info/Elements/x/P00008> ;
        reg:name                  "kapcsolódóCsaládPéldány"@hu ;
        rdfs:label                "van kapcsolódó családja (példány)"@hu ;
        skos:definition           "Egy példányt hozzákapcsol egy családhoz, amely egy éppen leírt példányhoz kötődik."@hu ;
        reg:hasUnconstrained      <http://rdaregistry.info/Elements/u/P61008> ;
        reg:hasSubproperty        <http://rdaregistry.info/Elements/i/P40145> ;
        reg:hasSubproperty        <http://rdaregistry.info/Elements/i/P40146> ;
        reg:hasSubproperty        <http://rdaregistry.info/Elements/i/P40147> ;
        reg:hasSubproperty        <http://rdaregistry.info/Elements/i/P40148> ;
        reg:hasSubproperty        <http://rdaregistry.info/Elements/i/P40151> ;
        reg:hasSubproperty        <http://rdaregistry.info/Elements/i/P40152> ;
        reg:hasSubproperty        <http://rdaregistry.info/Elements/i/P40158> ;
        reg:hasSubproperty        <http://rdaregistry.info/Elements/i/P40159> ;
        reg:hasSubproperty        <http://rdaregistry.info/Elements/i/P40160> ;
        rdakit:toolkitLabel       "famille en relation avec un item"@fr ;
        rdakit:toolkitDefinition  "Famille qui est associée à un item."@fr .

<http://rdaregistry.info/Elements/i/P40046>
        rdfs:isDefinedBy          <http://rdaregistry.info/Elements/i/> ;
        reg:status                <http://metadataregistry.org/uri/RegStatus/1001> ;
        reg:name                  "relatedItemOfItem"@en ;
        rdfs:label                "has related item of item"@en ;
        skos:definition           "Relates an item to an item that is associated with an item."@en ;
        rdf:type                  rdf:Property ;
        rdfs:domain               <http://rdaregistry.info/Elements/c/C10003> ;
        reg:hasSubproperty        <http://rdaregistry.info/Elements/i/P40053> ;
        reg:lexicalAlias          <http://rdaregistry.info/Elements/i/relatedItemOfItem.en> ;
        reg:hasSubproperty        <http://rdaregistry.info/Elements/i/P40051> ;
        reg:hasSubproperty        <http://rdaregistry.info/Elements/i/P40052> ;
        reg:hasSubproperty        <http://rdaregistry.info/Elements/i/P40054> ;
        reg:hasSubproperty        <http://rdaregistry.info/Elements/i/object/P40046> ;
        rdfs:label                "har relaterat exemplar"@sv ;
        rdakit:toolkitLabel       "relaterat exemplar"@sv ;
        rdfs:subPropertyOf        <http://rdaregistry.info/Elements/i/P40068> ;
        reg:hasUnconstrained      <http://rdaregistry.info/Elements/u/P60313> ;
        reg:name                  "bảnCóLiênQuanCủaBản"@vi ;
        rdfs:label                "có bản có liên quan (bản)"@vi ;
        skos:definition           "Liên kết bản với bản liên quan tới bản đang được mô tả."@vi ;
        reg:name                  "relateretEksemplarEksemplar"@da ;
        rdfs:label                "har relateret eksemplar (eksemplar)"@da ;
        reg:lexicalAlias          <http://rdaregistry.info/Elements/i/relateretEksemplarEksemplar.da> ;
        skos:definition           "Relaterer et eksemplar til et eksemplar, der er relateret til det eksemplar der beskrives."@da ;
        reg:name                  "σχετικόΑντίτυποΜεΑντίτυπο"@el ;
        rdfs:label                "έχει σχετικό αντίτυπο (αντίτυπο)"@el ;
        reg:lexicalAlias          <http://rdaregistry.info/Elements/i/σχετικόΑντίτυποΜεΑντίτυπο.el> ;
        skos:definition           "Συνδέει ένα αντίτυπο με ένα αντίτυπο που συνδέεται με το περιγραφόμενο αντίτυπο."@el ;
        rdfs:label                "té com a ítem relacionat (ítem)"@ca ;
        skos:definition           "Relaciona un item amb un item associat amb un ítem que es descriu."@ca ;
        reg:name                  "kappaleeseenLiittyvaKappale"@fi ;
        rdfs:label                "kappaleeseen liittyvä kappale"@fi ;
        reg:lexicalAlias          <rdaa:kappaleeseenLiittyvaKappale.fi> ;
        skos:definition           "Liittää kappaleen kappaleeseen, joka liittyy kuvailun kohteena olevaan kappaleeseen."@fi ;
        reg:name                  "itemEnRelationItem"@fr ;
        rdfs:label                "a pour item en relation avec un item"@fr ;
        reg:lexicalAlias          <http://rdaregistry.info/Elements/i/itemEnRelationAvecUnItem.fr> ;
        skos:definition           "Met un item en relation avec un item qui est associé à un item."@fr ;
        rdakit:toolkitLabel       "related item of item"@en ;
        rdakit:toolkitDefinition  "An item that is associated with an item."@en ;
        rdakit:hasElementType     "1" ;
        rdfs:subPropertyOf        <http://rdaregistry.info/Elements/x/P00005> ;
        reg:name                  "PéldánykapcsolódóPéldánya"@hu ;
        rdfs:label                "van kapcsolódó példánya (példány)"@hu ;
        skos:definition           "Egy példányt hozzákapcsol egy olyan példányhoz, amely kötődik egy éppen leírt példányhoz. "@hu ;
        reg:hasSubproperty        <http://rdaregistry.info/Elements/i/datatype/P40046> ;
        rdakit:toolkitLabel       "item en relation avec un item"@fr ;
        rdakit:toolkitDefinition  "Item qui est associé à un item."@fr ;
        skos:altLabel             "whole-part item relationship"@en .

<http://rdaregistry.info/Elements/i/P40071>
        rdfs:isDefinedBy          <http://rdaregistry.info/Elements/i/> ;
        reg:status                <http://metadataregistry.org/uri/RegStatus/1001> ;
        rdfs:subPropertyOf        <http://rdaregistry.info/Elements/i/P40068> ;
        rdf:type                  rdf:Property ;
        reg:name                  "relatedManifestationOfItem"@en ;
        rdfs:label                "has related manifestation of item"@en ;
        reg:lexicalAlias          <http://rdaregistry.info/Elements/i/relatedManifestationOfItem.en> ;
        skos:definition           "Relates an item to a manifestation that is associated with an item."@en ;
        rdfs:domain               <http://rdaregistry.info/Elements/c/C10003> ;
        reg:hasUnconstrained      <http://rdaregistry.info/Elements/u/P60313> ;
        reg:hasSubproperty        <http://rdaregistry.info/Elements/i/datatype/P40071> ;
        reg:hasSubproperty        <http://rdaregistry.info/Elements/i/object/P40071> ;
        reg:name                  "bảnBiểuThịCóLiênQuan"@vi ;
        rdfs:label                "có biểu thị có liên quan (bản)"@vi ;
        skos:definition           "Liên kết bản với thực biểu hiện liên quan với bản đang được mô tả."@vi ;
        reg:name                  "relateretManifestationEksemplar"@da ;
        rdfs:label                "har relateteret manifestation (eksemplar)"@da ;
        reg:lexicalAlias          <http://rdaregistry.info/Elements/i/relateretManifestationEksemplar.da> ;
        skos:definition           "Relaterer et eksemplar til en manifestation, der er knyttet til et beskrevet eksempar."@da ;
        reg:name                  "σχετικήΕκδήλωσηΑντιτύπου"@el ;
        rdfs:label                "έχει σχετική εκδήλωση (αντίτυπο)"@el ;
        reg:lexicalAlias          <http://rdaregistry.info/Elements/i/σχετικήΕκδήλωσηΑντιτύπου.el> ;
        skos:definition           "Συνδέει ένα αντίτυπο με μια εκδήλωση που συνδέεται με ένα περιγραφόμενο αντίτυπο."@el ;
        rdfs:label                "té com a manifestació relacionada (ítem)"@ca ;
        skos:definition           "Relaciona un item amb una manifestació associada amb un ítem que es descriu."@ca ;
        reg:name                  "kappaleeseenLiittyvaManifestaatio"@fi ;
        rdfs:label                "kappaleeseen liittyvä manifestaatio"@fi ;
        reg:lexicalAlias          <rdaa:kappaleeseenLiittyvaManifestaatio.fi> ;
        reg:name                  "manifestationEnRelationItem"@fr ;
        rdfs:label                "a pour manifestation en relation avec un item"@fr ;
        reg:lexicalAlias          <http://rdaregistry.info/Elements/i/manifestationEnRelationAvecUnItem.fr> ;
        skos:definition           "Met un item en relation avec une manifestation qui est associée à un item."@fr ;
        rdakit:toolkitLabel       "related manifestation of item"@en ;
        rdakit:toolkitDefinition  "A manifestation that is associated with an item."@en ;
        reg:hasSubproperty        <http://rdaregistry.info/Elements/i/P40049> ;
        rdakit:hasElementType     "1" ;
        rdfs:subPropertyOf        <http://rdaregistry.info/Elements/x/P00004> ;
        reg:name                  "kapcsolódóMegjelenésiformaPéldány"@hu ;
        rdfs:label                "van kapcsolódó megjelenési formája (példány)"@hu ;
        skos:definition           "Egy példányt hozzákapcsol egy olyan megjelenési formához, amely egy éppen leírt példányhoz kötődik."@hu ;
        reg:hasSubproperty        <http://rdaregistry.info/Elements/i/P40092> ;
        rdakit:toolkitLabel       "manifestation en relation avec un item"@fr ;
        rdakit:toolkitDefinition  "Manifestation qui est associée à un item."@fr .

<http://rdaregistry.info/Elements/i/P40079>
        rdfs:isDefinedBy          <http://rdaregistry.info/Elements/i/> ;
        reg:status                <http://metadataregistry.org/uri/RegStatus/1001> ;
        rdfs:subPropertyOf        <http://rdaregistry.info/Elements/i/P40068> ;
        rdf:type                  rdf:Property ;
        reg:name                  "relatedNomenOfItem"@en ;
        rdfs:label                "has related nomen of item"@en ;
        reg:lexicalAlias          <http://rdaregistry.info/Elements/i/relatedNomenOfItem.en> ;
        skos:definition           "Relates an item to a nomen that is associated with an item."@en ;
        rdfs:domain               <http://rdaregistry.info/Elements/c/C10003> ;
        reg:hasSubproperty        <http://rdaregistry.info/Elements/i/datatype/P40079> ;
        reg:hasSubproperty        <http://rdaregistry.info/Elements/i/object/P40079> ;
        reg:name                  "bảnDanhPhápCóLiênQuan"@vi ;
        rdfs:label                "có danh pháp có liên quan (bản)"@vi ;
        skos:definition           "Liên kết bản với danh pháp liên quan với bản đang được mô tả."@vi ;
        reg:name                  "relateretNomenEksemplar"@da ;
        rdfs:label                "har relateret nomen (eksemplar)"@da ;
        reg:lexicalAlias          <http://rdaregistry.info/Elements/i/relateretNomenEksemplar.da> ;
        skos:definition           "Relaterer et eksemplar til et nomen, der er knyttet til et beskrevet eksemplar."@da ;
        reg:name                  "σχετικόΌνομαΑντιτύπου"@el ;
        rdfs:label                "έχει σχετικό όνομα (αντίτυπο)"@el ;
        reg:lexicalAlias          <http://rdaregistry.info/Elements/i/σχετικόΌνομαΑντιτύπου.el> ;
        skos:definition           "Συνδέει ένα αντίτυπο με ένα όνομα που συνδέεται με ένα περιγραφόμενο αντίτυπο."@el ;
        rdfs:label                "té com a nomen relacionat (ítem)"@ca ;
        skos:definition           "Relaciona un item amb un nomen associat amb un ítem que es descriu."@ca ;
        reg:name                  "kappaleeseenLiittyvaNomen"@fi ;
        rdfs:label                "kappaleeseen liittyvä nomen"@fi ;
        reg:lexicalAlias          <rdaa:kappaleeseenLiittyvaNomen.fi> ;
        reg:name                  "nomenEnRelationItem"@fr ;
        rdfs:label                "a pour nomen en relation avec un item"@fr ;
        reg:lexicalAlias          <http://rdaregistry.info/Elements/i/nomenEnRelationAvecUnItem.fr> ;
        skos:definition           "Met un item en relation avec un nomen qui est associé à un item."@fr ;
        rdakit:toolkitLabel       "related nomen of item"@en ;
        rdakit:toolkitDefinition  "A nomen that is associated with an item."@en ;
        rdakit:hasElementType     "1" ;
        rdfs:subPropertyOf        <http://rdaregistry.info/Elements/x/P00013> ;
        reg:name                  "kapcsolódóNomenPéldány"@hu ;
        rdfs:label                "van kapcsolódó nomenje (példány)"@hu ;
        skos:definition           "Egy példányt hozzákapcsol egy nomenhez, amely egy épp leírt példányhoz kötődik."@hu ;
        reg:hasUnconstrained      <http://rdaregistry.info/Elements/u/P61023> ;
        reg:hasSubproperty        <http://rdaregistry.info/Elements/i/P40081> ;
        rdakit:toolkitLabel       "nomen en relation avec un item"@fr ;
        rdakit:toolkitDefinition  "Nomen qui est associé à un item."@fr .

<http://rdaregistry.info/Elements/i/P40073>
        rdfs:isDefinedBy          <http://rdaregistry.info/Elements/i/> ;
        reg:status                <http://metadataregistry.org/uri/RegStatus/1001> ;
        rdfs:subPropertyOf        <http://rdaregistry.info/Elements/i/P40072> ;
        rdf:type                  rdf:Property ;
        reg:name                  "relatedPersonOfItem"@en ;
        rdfs:label                "has related person of item"@en ;
        reg:lexicalAlias          <http://rdaregistry.info/Elements/i/relatedPersonOfItem.en> ;
        skos:definition           "Relates an item to a person who is associated with an item."@en ;
        rdfs:domain               <http://rdaregistry.info/Elements/c/C10003> ;
        reg:hasSubproperty        <http://rdaregistry.info/Elements/i/datatype/P40073> ;
        reg:hasSubproperty        <http://rdaregistry.info/Elements/i/object/P40073> ;
        reg:name                  "bảnCáNhânCóLiênQuan"@vi ;
        rdfs:label                "có cá nhân có liên quan (bản)"@vi ;
        skos:definition           "Liên kết bản với cá nhân liên quan với bản đang được mô tả."@vi ;
        reg:name                  "relateretPersonEksemplar"@da ;
        rdfs:label                "har relateret person (eksemplar)"@da ;
        reg:lexicalAlias          <http://rdaregistry.info/Elements/i/relateretPersonEksemplar.da> ;
        skos:definition           "Relaterer et eksemplar til en person, der er knyttet til et beskrevet eksemplar."@da ;
        reg:name                  "σχετικόΦυσικόΠρόσωποΑντιτύπου"@el ;
        rdfs:label                "έχει σχετικό φυσικό πρόσωπο (αντίτυπο)"@el ;
        reg:lexicalAlias          <http://rdaregistry.info/Elements/i/σχετικόΦυσικόΠρόσωποΑντιτύπου.el> ;
        skos:definition           "Συνδέει ένα αντίτυπο με ένα φυσικό πρόσωπο που συνδέεται με ένα περιγραφόμενο αντίτυπο."@el ;
        rdfs:label                "té com a persona relacionada (ítem)"@ca ;
        skos:definition           "Relaciona un item amb una persona associada amb un ítem que es descriu."@ca ;
        reg:name                  "kappaleeseenLiittyvaHenkilo"@fi ;
        rdfs:label                "kappaleeseen liittyvä henkilö"@fi ;
        reg:lexicalAlias          <rdaa:kappaleeseenLiittyvaHenkilo.fi> ;
        reg:name                  "personneEnRelationItem"@fr ;
        rdfs:label                "a pour personne en relation avec un item"@fr ;
        reg:lexicalAlias          <http://rdaregistry.info/Elements/i/personneEnRelationAvecUnItem.fr> ;
        skos:definition           "Met un item en relation avec une personne qui est associée à un item."@fr ;
        rdakit:toolkitLabel       "related person of item"@en ;
        rdakit:toolkitDefinition  "A person who is associated with an item."@en ;
        rdakit:hasElementType     "1" ;
        rdfs:subPropertyOf        <http://rdaregistry.info/Elements/x/P00007> ;
        reg:name                  "kapcsolódóSzemélyPéldány"@hu ;
        rdfs:label                "van kapcsolódó személye (példány)"@hu ;
        skos:definition           "Egy példányt hozzákapcsol egy személyhez, aki egy éppen leírt példányhoz kötődik."@hu ;
        reg:hasUnconstrained      <http://rdaregistry.info/Elements/u/P61008> ;
        reg:hasSubproperty        <http://rdaregistry.info/Elements/i/P40097> ;
        reg:hasSubproperty        <http://rdaregistry.info/Elements/i/P40098> ;
        reg:hasSubproperty        <http://rdaregistry.info/Elements/i/P40099> ;
        reg:hasSubproperty        <http://rdaregistry.info/Elements/i/P40100> ;
        reg:hasSubproperty        <http://rdaregistry.info/Elements/i/P40103> ;
        reg:hasSubproperty        <http://rdaregistry.info/Elements/i/P40104> ;
        reg:hasSubproperty        <http://rdaregistry.info/Elements/i/P40110> ;
        reg:hasSubproperty        <http://rdaregistry.info/Elements/i/P40111> ;
        reg:hasSubproperty        <http://rdaregistry.info/Elements/i/P40112> ;
        rdakit:toolkitLabel       "personne en relation avec un item"@fr ;
        rdakit:toolkitDefinition  "Personne qui est associée à un item."@fr .

<http://rdaregistry.info/Elements/i/P40077>
        rdfs:isDefinedBy          <http://rdaregistry.info/Elements/i/> ;
        reg:status                <http://metadataregistry.org/uri/RegStatus/1001> ;
        rdfs:subPropertyOf        <http://rdaregistry.info/Elements/i/P40068> ;
        rdf:type                  rdf:Property ;
        reg:name                  "relatedPlaceOfItem"@en ;
        rdfs:label                "has related place of item"@en ;
        reg:lexicalAlias          <http://rdaregistry.info/Elements/i/relatedPlaceOfItem.en> ;
        skos:definition           "Relates an item to a place that is associated with an item."@en ;
        rdfs:domain               <http://rdaregistry.info/Elements/c/C10003> ;
        reg:hasSubproperty        <http://rdaregistry.info/Elements/i/datatype/P40077> ;
        reg:hasSubproperty        <http://rdaregistry.info/Elements/i/object/P40077> ;
        reg:name                  "bảnĐịaĐiểmCóLiênQuan"@vi ;
        rdfs:label                "có địa điểm có liên quan (bản)"@vi ;
        skos:definition           "Liên kết bản với địa điểm liên quan với bản đang được mô tả."@vi ;
        reg:name                  "relateretStedEksemplar"@da ;
        rdfs:label                "har relateret sted (eksemplar)"@da ;
        reg:lexicalAlias          <http://rdaregistry.info/Elements/i/relateretStedEksemplar.da> ;
        skos:definition           "Relaterer et eksemplar til et sted, der er knyttet til et beskrevet eksemplar."@da ;
        reg:name                  "σχετικόςΤόποςΑντιτύπου"@el ;
        rdfs:label                "έχει σχετικό τόπο (αντίτυπο)"@el ;
        reg:lexicalAlias          <http://rdaregistry.info/Elements/i/σχετικόςΤόποςΑντιτύπου.el> ;
        skos:definition           "Συνδέει ένα αντίτυπο με έναν τόπο που συνδέεται με ένα περιγραφόμενο αντίτυπο."@el ;
        rdfs:label                "té com a lloc relacionat (ítem)"@ca ;
        skos:definition           "Relaciona un item amb un lloc associat amb un ítem que es descriu."@ca ;
        reg:name                  "kappaleeseenLiittyvaPaikka"@fi ;
        rdfs:label                "kappaleeseen liittyvä paikka"@fi ;
        reg:lexicalAlias          <rdaa:kappaleeseenLiittyvaPaikka.fi> ;
        reg:name                  "lieuEnRelationItem"@fr ;
        rdfs:label                "a pour lieu en relation avec un item"@fr ;
        reg:lexicalAlias          <http://rdaregistry.info/Elements/i/lieuEnRelationAvecUnItem.fr> ;
        skos:definition           "Met un item en relation avec un lieu qui est associé à un item."@fr ;
        rdakit:toolkitLabel       "related place of item"@en ;
        rdakit:toolkitDefinition  "A place that is associated with an item."@en ;
        rdakit:hasElementType     "1" ;
        rdfs:subPropertyOf        <http://rdaregistry.info/Elements/x/P00010> ;
        reg:name                  "kapcsolódóHelyPéldány"@hu ;
        rdfs:label                "van kapcsolódó helye (példány)"@hu ;
        skos:definition           "Egy példányt hozzákapcsol egy helyhez, amely egy éppen leírt példányhoz kötődik."@hu ;
        reg:hasUnconstrained      <http://rdaregistry.info/Elements/u/P61014> ;
        rdakit:toolkitLabel       "lieu en relation avec un item"@fr ;
        rdakit:toolkitDefinition  "Lieu qui est associé à un item."@fr .

<http://rdaregistry.info/Elements/i/P40068>
        rdfs:isDefinedBy          <http://rdaregistry.info/Elements/i/> ;
        reg:status                <http://metadataregistry.org/uri/RegStatus/1001> ;
        rdfs:subPropertyOf        <http://rdaregistry.info/Elements/i/P40095> ;
        rdf:type                  rdf:Property ;
        reg:name                  "relatedRDAEntityOfItem"@en ;
        rdfs:label                "has related RDA entity of item"@en ;
        reg:lexicalAlias          <http://rdaregistry.info/Elements/i/relatedRDAEntityOfItem.en> ;
        skos:definition           "Relates an item to an RDA entity that is associated with an item."@en ;
        rdfs:domain               <http://rdaregistry.info/Elements/c/C10003> ;
        reg:hasSubproperty        <http://rdaregistry.info/Elements/i/P40046> ;
        reg:hasSubproperty        <http://rdaregistry.info/Elements/i/P40069> ;
        reg:hasSubproperty        <http://rdaregistry.info/Elements/i/P40070> ;
        reg:hasSubproperty        <http://rdaregistry.info/Elements/i/P40071> ;
        reg:hasSubproperty        <http://rdaregistry.info/Elements/i/P40072> ;
        reg:hasSubproperty        <http://rdaregistry.info/Elements/i/P40077> ;
        reg:hasSubproperty        <http://rdaregistry.info/Elements/i/P40078> ;
        reg:hasSubproperty        <http://rdaregistry.info/Elements/i/P40079> ;
        reg:hasSubproperty        <http://rdaregistry.info/Elements/i/datatype/P40068> ;
        reg:hasSubproperty        <http://rdaregistry.info/Elements/i/object/P40068> ;
        reg:name                  "bảnThựcThểCóLiênQuan"@vi ;
        rdfs:label                "có thực thể có liên quan (bản)"@vi ;
        skos:definition           "Liên kết bản với thực thể liên quan với bản đang được mô tả."@vi ;
        reg:name                  "relateretEntitetEksemplar"@da ;
        rdfs:label                "har relateret entitet (eksemplar)"@da ;
        reg:lexicalAlias          <http://rdaregistry.info/Elements/i/relateretEntitetEksemplar.da> ;
        skos:definition           "Relaterer et eksemplar til en entitet, der er knyttet til et beskrevet eksemplar."@da ;
        reg:name                  "σχετικήΟντότηταΑντιτύπου"@el ;
        rdfs:label                "έχει σχετική οντότητα στο (αντίτυπο)"@el ;
        reg:lexicalAlias          <http://rdaregistry.info/Elements/i/σχετικήΟντότηταΑντιτύπου.el> ;
        skos:definition           "Συνδέει ένα αντίτυπο με μια οντότητα που συνδέεται με ένα περιγραφόμενο αντίτυπο."@el ;
        rdfs:label                "té com a entitat relacionada (ítem)"@ca ;
        skos:definition           "Relaciona un item amb una entitat associada amb un ítem que es descriu."@ca ;
        reg:name                  "kappaleeseenLiittyvaEntiteetti"@fi ;
        rdfs:label                "kappaleeseen liittyvä entiteetti"@fi ;
        reg:lexicalAlias          <rdaa:kappaleeseenLiittyvaEntiteetti.fi> ;
        reg:name                  "entitéEnRelationItem"@fr ;
        rdfs:label                "a pour entité RDA en relation avec un item"@fr ;
        reg:lexicalAlias          <http://rdaregistry.info/Elements/i/entitéRdaEnRelationAvecUnItem.fr> ;
        skos:definition           "Met un item en relation avec une entité RDA qui est associée à un item."@fr ;
        rdakit:toolkitLabel       "related RDA entity of item"@en ;
        rdakit:toolkitDefinition  "An RDA entity that is associated with an item."@en ;
        rdakit:hasElementType     "1" ;
        reg:name                  "kapcsolódóEntitásPéldány"@hu ;
        rdfs:label                "van kapcsolódó entitása (példány)"@hu ;
        skos:definition           "Egy példányt hozzákapcsol egy entitáshoz, amely egy éppen leírt példányhoz kötődik."@hu ;
        reg:hasUnconstrained      <http://rdaregistry.info/Elements/u/P61034> ;
        rdfs:subPropertyOf        <http://rdaregistry.info/Elements/x/P00001> ;
        rdakit:toolkitLabel       "entité RDA en relation avec un item"@fr ;
        rdakit:toolkitDefinition  "Entité RDA qui est associée à un item."@fr .

<http://rdaregistry.info/Elements/i/P40078>
        rdfs:isDefinedBy          <http://rdaregistry.info/Elements/i/> ;
        reg:status                <http://metadataregistry.org/uri/RegStatus/1001> ;
        rdfs:subPropertyOf        <http://rdaregistry.info/Elements/i/P40068> ;
        rdf:type                  rdf:Property ;
        reg:name                  "relatedTimespanOfItem"@en ;
        rdfs:label                "has related timespan of item"@en ;
        reg:lexicalAlias          <http://rdaregistry.info/Elements/i/relatedTimespanOfItem.en> ;
        skos:definition           "Relates an item to a timespan that is associated with an item."@en ;
        rdfs:domain               <http://rdaregistry.info/Elements/c/C10003> ;
        reg:hasSubproperty        <http://rdaregistry.info/Elements/i/datatype/P40078> ;
        reg:hasSubproperty        <http://rdaregistry.info/Elements/i/object/P40078> ;
        reg:name                  "bảnKhoảngThờiGianCóLiênQuan"@vi ;
        rdfs:label                "có khoảng thời gian có liên quan (bản)"@vi ;
        skos:definition           "Liên kết bản với khoảng thời gian liên quan với bản đang được mô tả."@vi ;
        reg:name                  "relateretTidsforløbEksemplar"@da ;
        rdfs:label                "har relateret tidsforløb (eksemplar)"@da ;
        reg:lexicalAlias          <http://rdaregistry.info/Elements/i/relateretTidsforløbEksemplar.da> ;
        skos:definition           "Relaterer et eksemplar til en periode, der er knyttet til et beskrevet eksemplar."@da ;
        reg:name                  "σχετικόΧρονικόΔιάστημαΑντιτύπου"@el ;
        rdfs:label                "έχει σχετικό χρονικό διάστημα (αντίτυπο)"@el ;
        reg:lexicalAlias          <http://rdaregistry.info/Elements/i/σχετικόΧρονικόΔιάστημαΑντιτύπου.el> ;
        skos:definition           "Συνδέει ένα αντίτυπο με το χρονικό διάστημα που συνδέεται με ένα περιγραφόμενο αντίτυπο."@el ;
        rdfs:label                "té com a període de temps relacionat (ítem)"@ca ;
        skos:definition           "Relaciona un item amb un període de temps associat amb un ítem que es descriu."@ca ;
        reg:name                  "kappaleeseenLiittyvaAjanjakso"@fi ;
        rdfs:label                "kappaleeseen liittyvä ajanjakso"@fi ;
        reg:lexicalAlias          <rdaa:kappaleeseenLiittyvaAjanjakso.fi> ;
        reg:name                  "lapsDeTempsEnRelationItem"@fr ;
        rdfs:label                "a pour laps de temps en relation avec un item"@fr ;
        reg:lexicalAlias          <http://rdaregistry.info/Elements/i/lapsDeTempsEnRelationAvecUnItem.fr> ;
        skos:definition           "Met un item en relation avec un laps de temps qui est associé à un item."@fr ;
        rdakit:toolkitLabel       "related timespan of item"@en ;
        rdakit:toolkitDefinition  "A timespan that is associated with an item."@en ;
        rdakit:hasElementType     "1" ;
        rdfs:subPropertyOf        <http://rdaregistry.info/Elements/x/P00011> ;
        reg:name                  "kapcsolódóIdőtartamPéldány"@hu ;
        rdfs:label                "van kapcsolódó időtartama (példány)"@hu ;
        skos:definition           "Egy példányt hozzákapcsol egy időtartamhoz, amely egy éppen leírt példányhoz kötődik."@hu ;
        reg:hasUnconstrained      <http://rdaregistry.info/Elements/u/P61020> ;
        rdakit:toolkitLabel       "laps de temps en relation avec un item"@fr ;
        rdakit:toolkitDefinition  "Laps de temps qui est associé à un item."@fr .

<http://rdaregistry.info/Elements/i/P40069>
        rdfs:isDefinedBy          <http://rdaregistry.info/Elements/i/> ;
        reg:status                <http://metadataregistry.org/uri/RegStatus/1001> ;
        rdfs:subPropertyOf        <http://rdaregistry.info/Elements/i/P40068> ;
        rdf:type                  rdf:Property ;
        reg:name                  "relatedWorkOfItem"@en ;
        rdfs:label                "has related work of item"@en ;
        reg:lexicalAlias          <http://rdaregistry.info/Elements/i/relatedWorkOfItem.en> ;
        skos:definition           "Relates an item to a work that is associated with an item."@en ;
        rdfs:domain               <http://rdaregistry.info/Elements/c/C10003> ;
        reg:hasUnconstrained      <http://rdaregistry.info/Elements/u/P60313> ;
        reg:hasSubproperty        <http://rdaregistry.info/Elements/i/datatype/P40069> ;
        reg:hasSubproperty        <http://rdaregistry.info/Elements/i/object/P40069> ;
        reg:name                  "bảnTácPhẩmCóLiênQuan"@vi ;
        rdfs:label                "có tác phẩm có liên quan (bản)"@vi ;
        skos:definition           "Liên kết bản với tác phẩm liên quan với bản đang được mô tả."@vi ;
        reg:name                  "relateretVærkEksemplar"@da ;
        rdfs:label                "har relateret værk (eksemplar)"@da ;
        reg:lexicalAlias          <http://rdaregistry.info/Elements/i/relateretVærkEksemplar.da> ;
        skos:definition           "Relaterer et eksemplar til et værk, der er knyttet til et beskrevet eksemplar."@da ;
        reg:name                  "σχετικόΈργοΑντιτύπου"@el ;
        rdfs:label                "έχει σχετικό έργο (αντίτυπο)"@el ;
        reg:lexicalAlias          <http://rdaregistry.info/Elements/i/σχετικόΈργοΑντιτύπου.el> ;
        skos:definition           "Συνδέει ένα αντίτυπο με ένα έργο που συνδέεται με ένα περιγραφόμενο αντίτυπο."@el ;
        rdfs:label                "té com a obra relacionada (ítem)"@ca ;
        skos:definition           "Relaciona un item amb una obra associada amb un ítem que es descriu."@ca ;
        reg:name                  "kappaleeseenLiittyvaTeos"@fi ;
        rdfs:label                "kappaleeseen liittyvä teos"@fi ;
        reg:lexicalAlias          <rdaa:kappaleeseenLiittyvaTeos.fi> ;
        reg:name                  "œuvreEnRelationItem"@fr ;
        rdfs:label                "a pour œuvre en relation avec un item"@fr ;
        reg:lexicalAlias          <http://rdaregistry.info/Elements/i/œuvreEnRelationAvecUnItem.fr> ;
        skos:definition           "Met un item en relation avec une œuvre qui est associée à un item."@fr ;
        rdakit:toolkitLabel       "related work of item"@en ;
        rdakit:toolkitDefinition  "A work that is associated with an item."@en ;
        reg:hasSubproperty        <http://rdaregistry.info/Elements/i/P40061> ;
        rdakit:hasElementType     "1" ;
        rdfs:subPropertyOf        <http://rdaregistry.info/Elements/x/P00002> ;
        reg:name                  "kapcsolódóMűPéldány"@hu ;
        rdfs:label                "van kapcsolódó műve (példány)"@hu ;
        skos:definition           "Egy példányt hozzákapcsol egy olyan műhöz, amely egy éppen leírt példányhoz kötődik. "@hu ;
        reg:hasSubproperty        <http://rdaregistry.info/Elements/i/P40094> ;
        rdakit:toolkitLabel       "œuvre en relation avec un item"@fr ;
        rdakit:toolkitDefinition  "Œuvre qui est associée à un item."@fr .

<http://rdaregistry.info/Elements/i/P40091>
        rdfs:isDefinedBy          <http://rdaregistry.info/Elements/i/> ;
        reg:status                <http://metadataregistry.org/uri/RegStatus/1001> ;
        rdfs:label                "is reprinted as item"@en ;
        rdf:type                  rdf:Property ;
        reg:name                  "reprintedAsItem"@en ;
        reg:lexicalAlias          <http://rdaregistry.info/Elements/i/reprintedAsItem.en> ;
        rdfs:domain               <http://rdaregistry.info/Elements/c/C10003> ;
        skos:definition           "Relates an item to a manifestation that is a reissue of an item that exemplifies another printed manifestation."@en ;
        rdfs:subPropertyOf        <http://rdaregistry.info/Elements/i/P40092> ;
        rdakit:toolkitLabel       "reprinted as item"@en ;
        rdakit:toolkitDefinition  "A manifestation that is a reissue of an item that exemplifies another printed manifestation."@en ;
        reg:hasUnconstrained      <http://rdaregistry.info/Elements/u/P60271> ;
        rdakit:hasElementType     "2" ;
        reg:hasSubproperty        <http://rdaregistry.info/Elements/i/datatype/P40091> ;
        rdfs:label                "est réimprimé comme un item"@fr ;
        skos:definition           "Met un item en relation avec une manifestation qui est une réédition d’un item représentant une autre manifestation imprimée."@fr ;
        rdakit:toolkitLabel       "réimprimé comme un item"@fr ;
        rdakit:toolkitDefinition  "Manifestation qui est une réédition d’un item représentant une autre manifestation imprimée."@fr ;
        reg:lexicalAlias          <http://rdaregistry.info/Elements/i/réimpriméCommeUnItem.fr> .

<http://rdaregistry.info/Elements/i/P40060>
        rdfs:isDefinedBy          <http://rdaregistry.info/Elements/i/> ;
        reg:status                <http://metadataregistry.org/uri/RegStatus/1008> ;
        rdf:type                  rdf:Property ;
        rdfs:domain               <http://rdaregistry.info/Elements/c/C10003> ;
        reg:hasUnconstrained      <http://rdaregistry.info/Elements/u/P60271> ;
        rdfs:label                "est réimprimé comme (item)"@fr ;
        skos:definition           "Met un item en relation avec un item qui est une réédition d’un item représentant une autre manifestation imprimée."@fr ;
        rdakit:toolkitLabel       "réimprimé comme (item)"@fr ;
        rdakit:toolkitDefinition  "Item qui est une réédition d’un item représentant une autre manifestation imprimée."@fr ;
        rdakit:toolkitLabel       "reimpreso como (ítem)"@es ;
        rdakit:toolkitDefinition  "Un ítem que es una reedición de un ítem que ejemplifica otra manifestación impresa."@es ;
        rdfs:subPropertyOf        <http://rdaregistry.info/Elements/i/P40055> ;
        rdakit:instructionNumber  "24.5" ;
        reg:hasSubproperty        <http://rdaregistry.info/Elements/i/object/P40060> ;
        reg:name                  "đượcInLạiNhưLàBản"@vi ;
        rdfs:label                "được in lại như là (bản)"@vi ;
        skos:definition           "Liên kết bản với bản là bản công bố lại của bản thể hiện biểu thị được in khác."@vi ;
        rdakit:toolkitLabel       "được in lại như là (bản)"@vi ;
        rdakit:toolkitDefinition  "Bản là bản công bố lại của bản thể hiện biểu thị được in khác."@vi ;
        reg:name                  "genoptryktSom"@da ;
        rdfs:label                "er genoptryk som (eksemplar)"@da ;
        reg:lexicalAlias          <http://rdaregistry.info/Elements/i/genoptryktSom.da> ;
        skos:definition           "Relaterer et eksemplar til et eksemplar, der er en genudgivelse af et eksemplar, som eksemplificerer en anden trykt manifestation."@da ;
        rdakit:toolkitLabel       "genoptrykt som (eksemplar)"@da ;
        rdakit:toolkitDefinition  "Eksemplar, der er en genudgivelse af et eksemplar, som eksemplificerer en anden trykt manifestation."@da ;
        rdfs:label                "ist nachgedruckt als (Exemplar)"@de ;
        skos:definition           "Setzt ein Exemplar mit einem Exemplar, das eine Neuausgabe eines Exemplars ist, das eine andere gedruckte Manifestation darstellt, in Beziehung."@de ;
        rdakit:toolkitLabel       "Nachgedruckt als (Exemplar)"@de ;
        rdakit:toolkitDefinition  "Ein Exemplar, das eine Neuausgabe eines Exemplars ist, das eine andere gedruckte Manifestation darstellt."@de ;
        reg:name                  "ανατυπωμένοΩςΑντίτυπο"@el ;
        rdfs:label                "είναι ανατυπωμένο ως (αντίτυπο)"@el ;
        reg:lexicalAlias          <http://rdaregistry.info/Elements/i/ανατυπωμένοΩςΑντίτυπο.el> ;
        skos:definition           "Συνδέει ένα αντίτυπο με ένα αντίτυπο το οποίο είναι επανέκδοση ενός αντιτύπου που υλοποιεί κάποια άλλη έντυπη εκδήλωση."@el ;
        rdakit:toolkitLabel       "ανατυπωμένο ως (αντίτυπο)"@el ;
        rdakit:toolkitDefinition  "Ένα αντίτυπο το οποίο είναι επανέκδοση ενός αντιτύπου που υλοποιεί κάποια άλλη έντυπη εκδήλωση."@el ;
        rdfs:label                "és reimprès com (ítem)"@ca ;
        skos:definition           "Relaciona un item amb un ítem que és una reimpressió d’un ítem que exemplifica una altra manifestació impresa."@ca ;
        rdakit:toolkitLabel       "reimprès com (ítem)"@ca ;
        rdakit:toolkitDefinition  "Ítem que és una reimpressió d’un ítem que exemplifica una altra manifestació impresa."@ca ;
        reg:name                  "uusintapainosKappale"@fi ;
        rdfs:label                "uusintapainos (kappale)"@fi ;
        reg:lexicalAlias          <rdaa:uusintapainosKappale.fi> ;
        skos:definition           "Liittää kappaleen kappaleeseen, joka on uusi painos toisesta samansisältöisestä manifestaatiosta."@fi ;
        rdakit:toolkitLabel       "uusintapainos (kappale)"@fi ;
        rdakit:toolkitDefinition  "Kappale, joka on uusi painos toisesta samansisältöisestä manifestaatiosta."@fi ;
        reg:name                  "réimpriméCommeItem"@fr ;
        reg:lexicalAlias          <http://rdaregistry.info/Elements/i/réimpriméCommeItem.fr> ;
        rdakit:toolkitLabel       "opptrykt som (eksemplar)"@no ;
        rdakit:toolkitDefinition  "Et eksemplar som er et opptrykk av et eksemplar som er et eksempel på en annen trykt manifestasjon."@no ;
        reg:hasSubproperty        <http://rdaregistry.info/Elements/i/datatype/P40060> .

<http://rdaregistry.info/Elements/i/P40038>
        rdfs:isDefinedBy          <http://rdaregistry.info/Elements/i/> ;
        reg:status                <http://metadataregistry.org/uri/RegStatus/1008> ;
        rdf:type                  rdf:Property ;
        rdfs:domain               <http://rdaregistry.info/Elements/c/C10003> ;
        rdfs:subPropertyOf        <http://rdaregistry.info/Elements/i/P40042> ;
        reg:hasUnconstrained      <http://rdaregistry.info/Elements/u/P60168> ;
        rdfs:label                "est une réimpression de (item)"@fr ;
        skos:definition           "Met un item en relation avec un item qui représente une manifestation imprimée servant de base à une réédition d’une manifestation."@fr ;
        rdakit:toolkitLabel       "réimpression de (item)"@fr ;
        rdakit:toolkitDefinition  "Item qui représente une manifestation imprimée servant de base à une réédition d’une manifestation."@fr ;
        rdakit:toolkitLabel       "reimpresión de (ítem)"@es ;
        rdakit:toolkitDefinition  "Un ítem que ejemplifica una manifestación impresa que se usa como base para una reedición de una manifestación."@es ;
        rdakit:instructionNumber  "24.5" ;
        reg:hasSubproperty        <http://rdaregistry.info/Elements/i/object/P40038> ;
        reg:name                  "táiBảnCủaBản"@vi ;
        rdfs:label                "là tái bản của (bản)"@vi ;
        skos:definition           "Liên kết bản với bản thể hiện biểu thị đã được in, được sử dụng như là cơ sở cho công bố lại biểu thị."@vi ;
        rdakit:toolkitLabel       "tái bản của (bản)"@vi ;
        rdakit:toolkitDefinition  "Bản thể hiện biểu thị đã được in, được sử dụng như là cơ sở cho công bố lại biểu thị."@vi ;
        reg:name                  "genudgivelseAfEksemplar"@da ;
        rdfs:label                "er genudgivelse af (eksemplar)"@da ;
        reg:lexicalAlias          <http://rdaregistry.info/Elements/i/genudgivelseAfEksemplar.da> ;
        skos:definition           "Relaterer et eksemplar til et eksemplar, der eksemplificerer en trykt manifestation, der er anvendt som grundlag for et genoptryk af en manifestation."@da ;
        rdakit:toolkitLabel       "genudgivelse af (eksemplar)"@da ;
        rdakit:toolkitDefinition  "Eksemplar, der eksemplificerer en trykt manifestation, der er anvendt som grundlag for et genoptryk af en manifestation."@da ;
        rdfs:label                "ist Nachdruck von (Exemplar)"@de ;
        skos:definition           "Setzt ein Exemplar mit einem Exemplar, das eine gedruckte Manifestation darstellt, die als Grundlage für eine Neuausgabe einer Manifestation verwendet wurde, in Beziehung."@de ;
        rdakit:toolkitLabel       "Nachdruck von (Exemplar)"@de ;
        rdakit:toolkitDefinition  "Ein Exemplar, das eine gedruckte Manifestation darstellt, die als Grundlage für eine Neuausgabe einer Manifestation verwendet wurde."@de ;
        reg:name                  "ανατύπωσηΤουΑντιτύπου"@el ;
        rdfs:label                "είναι ανατύπωση του (αντίτυπο)"@el ;
        reg:lexicalAlias          <http://rdaregistry.info/Elements/i/ανατύπωσηΤουΑντιτύπου.el> ;
        skos:definition           "Συνδέει ένα αντίτυπο με ένα αντίτυπο το οποίο αποτελεί παράδειγμα υλοποίησης μιας έντυπης εκδήλωσης η οποία χρησιμοποιείται ως η βάση για την επανέκδοση μιας εκδήλωσης."@el ;
        rdakit:toolkitLabel       "ανατύπωση του (αντίτυπο)"@el ;
        rdakit:toolkitDefinition  "Ένα αντίτυπο το οποίο αποτελεί παράδειγμα υλοποίησης μιας έντυπης εκδήλωσης, η οποία χρησιμοποιείται ως η βάση για την επανέκδοση μιας εκδήλωσης."@el ;
        rdfs:label                "és reimpressió de (ítem)"@ca ;
        skos:definition           "Relaciona un item amb un ítem que exemplifica una manifestació impresa que s’usa com a base d’una reimpressió d’una manifestació."@ca ;
        rdakit:toolkitLabel       "reimpressió de (ítem)"@ca ;
        rdakit:toolkitDefinition  "Ítem que exemplifica una manifestació impresa que s’usa com a base d’una reimpressió d’una manifestació."@ca ;
        reg:name                  "alkuperainenPainosKappale"@fi ;
        rdfs:label                "alkuperäinen painos (kappale)"@fi ;
        reg:lexicalAlias          <rdaa:alkuperainenPainosKappale.fi> ;
        skos:definition           "Liittää kappaleen kappaleeseen, joka edustaa julkaistua manifestaatiota, jonka pohjalta manifestaation uusi painos on tehty."@fi ;
        rdakit:toolkitLabel       "alkuperäinen painos (kappale)"@fi ;
        rdakit:toolkitDefinition  "Kappale, joka edustaa julkaistua manifestaatiota, jonka pohjalta manifestaation uusi painos on tehty."@fi ;
        reg:name                  "réimpressionDeItem"@fr ;
        reg:lexicalAlias          <http://rdaregistry.info/Elements/i/réimpressionDeItem.fr> ;
        rdakit:toolkitLabel       "opptrykk av (eksemplar)"@no ;
        rdakit:toolkitDefinition  "Et eksemplar som er et eksempel på en trykt manifestasjon som brukes som utgangspunkt for et opptrykk av en manifestasjon."@no ;
        reg:hasSubproperty        <http://rdaregistry.info/Elements/i/datatype/P40038> .

<http://rdaregistry.info/Elements/i/P40092>
        rdfs:isDefinedBy          <http://rdaregistry.info/Elements/i/> ;
        reg:status                <http://metadataregistry.org/uri/RegStatus/1001> ;
        rdfs:label                "is reproduced as item"@en ;
        rdf:type                  rdf:Property ;
        reg:name                  "reproducedAsItem"@en ;
        reg:lexicalAlias          <http://rdaregistry.info/Elements/i/reproducedAsItem.en> ;
        skos:definition           "Relates an item to a manifestation that reproduces an item that exemplifies another manifestation."@en ;
        rdfs:domain               <http://rdaregistry.info/Elements/c/C10003> ;
        rdfs:subPropertyOf        <http://rdaregistry.info/Elements/i/P40071> ;
        rdakit:toolkitLabel       "reproduced as item"@en ;
        rdakit:toolkitDefinition  "A manifestation that reproduces an item that exemplifies another manifestation."@en ;
        reg:hasUnconstrained      <http://rdaregistry.info/Elements/u/P60272> ;
        rdakit:hasElementType     "2" ;
        reg:hasSubproperty        <http://rdaregistry.info/Elements/i/datatype/P40092> ;
        reg:hasSubproperty        <http://rdaregistry.info/Elements/i/P40087> ;
        reg:hasSubproperty        <http://rdaregistry.info/Elements/i/P40088> ;
        reg:hasSubproperty        <http://rdaregistry.info/Elements/i/P40089> ;
        reg:hasSubproperty        <http://rdaregistry.info/Elements/i/P40091> ;
        rdfs:label                "est reproduit comme un item"@fr ;
        skos:definition           "Met un item en relation avec une manifestation qui reproduit un item représentant une autre manifestation."@fr ;
        rdakit:toolkitLabel       "reproduit comme un item"@fr ;
        rdakit:toolkitDefinition  "Manifestation qui reproduit un item représentant une autre manifestation."@fr ;
        reg:lexicalAlias          <http://rdaregistry.info/Elements/i/reproduitCommeUnItem.fr> .

<http://rdaregistry.info/Elements/i/P40055>
        rdfs:isDefinedBy          <http://rdaregistry.info/Elements/i/> ;
        reg:status                <http://metadataregistry.org/uri/RegStatus/1008> ;
        rdf:type                  rdf:Property ;
        rdfs:domain               <http://rdaregistry.info/Elements/c/C10003> ;
        reg:hasUnconstrained      <http://rdaregistry.info/Elements/u/P60272> ;
        rdfs:label                "est reproduit comme (item)"@fr ;
        skos:definition           "Met un item en relation avec un item qui reproduit un autre item."@fr ;
        rdakit:toolkitLabel       "reproduit comme (item)"@fr ;
        rdakit:toolkitDefinition  "Item qui reproduit un autre item."@fr ;
        rdakit:toolkitLabel       "reproducida como (ítem)"@es ;
        rdakit:toolkitDefinition  "Un ítem que reproduce otro ítem."@es ;
        rdfs:subPropertyOf        <http://rdaregistry.info/Elements/i/P40031> ;
        reg:hasSubproperty        <http://rdaregistry.info/Elements/i/P40056> ;
        reg:hasSubproperty        <http://rdaregistry.info/Elements/i/P40057> ;
        reg:hasSubproperty        <http://rdaregistry.info/Elements/i/P40058> ;
        reg:hasSubproperty        <http://rdaregistry.info/Elements/i/P40060> ;
        rdakit:instructionNumber  "24.5" ;
        reg:hasSubproperty        <http://rdaregistry.info/Elements/i/object/P40055> ;
        reg:name                  "đượcSaoChépNhưLàBản"@vi ;
        rdfs:label                "được sao chép như là (bản)"@vi ;
        skos:definition           "Liên kết bản với bản tạo lại bản khác."@vi ;
        rdakit:toolkitLabel       "được sao chép như là (bản)"@vi ;
        rdakit:toolkitDefinition  "Bản tạo lại bản khác."@vi ;
        reg:name                  "reproduceretSomEksemplar"@da ;
        rdfs:label                "er reproduceret som (eksemplar)"@da ;
        reg:lexicalAlias          <http://rdaregistry.info/Elements/i/reproduceretSomEksemplar.da> ;
        skos:definition           "Relaterer et eksemplar til et eksemplar, der reproducerer et andet eksemplar."@da ;
        rdakit:toolkitLabel       "reproduceret som (eksemplar)"@da ;
        rdakit:toolkitDefinition  "Eksemplar, der reproducerer et andet eksemplar."@da ;
        rdfs:label                "ist reproduziert als (Exemplar)"@de ;
        skos:definition           "Setzt ein Exemplar mit einem Exemplar, das ein anderes Exemplar reproduziert, in Beziehung."@de ;
        rdakit:toolkitLabel       "Reproduziert als (Exemplar)"@de ;
        rdakit:toolkitDefinition  "Ein Exemplar, das ein anderes Exemplar reproduziert."@de ;
        reg:name                  "αναπαραγόμενοΩςΑντίτυπο"@el ;
        rdfs:label                "έχει αναπαραχθεί ως (αντίτυπο)"@el ;
        reg:lexicalAlias          <http://rdaregistry.info/Elements/i/αναπαραγόμενοΩςΑντίτυπο.el> ;
        skos:definition           "Συνδέει ένα αντίτυπο με ένα αντίτυπο που αναπαράγει κάποιο άλλο αντίτυπο."@el ;
        rdakit:toolkitLabel       "έχει αναπαραχθεί ως (αντίτυπο)"@el ;
        rdakit:toolkitDefinition  "Ένα αντίτυπο που αναπαράγει κάποιο άλλο αντίτυπο."@el ;
        rdfs:label                "és reproduït com (ítem)"@ca ;
        skos:definition           "Relaciona un item amb un ítem que reprodueix un altre ítem."@ca ;
        rdakit:toolkitLabel       "reproduït com (ítem)"@ca ;
        rdakit:toolkitDefinition  "Ítem que reprodueix un altre ítem."@ca ;
        reg:name                  "jaljenteenaKappale"@fi ;
        rdfs:label                "jäljenteenä (kappale)"@fi ;
        reg:lexicalAlias          <rdaa:jaljenteenaKappale.fi> ;
        skos:definition           "Liittää kappaleen kappaleeseen, joka on jäljenne toisesta kappaleesta."@fi ;
        rdakit:toolkitLabel       "jäljenteenä (kappale)"@fi ;
        rdakit:toolkitDefinition  "Kappale, joka on jäljenne toisesta kappaleesta."@fi ;
        reg:name                  "reproduitCommeItem"@fr ;
        reg:lexicalAlias          <http://rdaregistry.info/Elements/i/reproduitCommeItem.fr> ;
        rdakit:toolkitLabel       "reprodusert som (eksemplar)"@no ;
        rdakit:toolkitDefinition  "Et eksemplar som reproduserer et annet eksemplar."@no ;
        reg:hasSubproperty        <http://rdaregistry.info/Elements/i/datatype/P40055> .

<http://rdaregistry.info/Elements/i/P40042>
        rdfs:isDefinedBy          <http://rdaregistry.info/Elements/i/> ;
        reg:status                <http://metadataregistry.org/uri/RegStatus/1008> ;
        rdf:type                  rdf:Property ;
        rdfs:domain               <http://rdaregistry.info/Elements/c/C10003> ;
        rdfs:subPropertyOf        <http://rdaregistry.info/Elements/i/P40031> ;
        reg:hasSubproperty        <http://rdaregistry.info/Elements/i/P40027> ;
        reg:hasSubproperty        <http://rdaregistry.info/Elements/i/P40038> ;
        reg:hasSubproperty        <http://rdaregistry.info/Elements/i/P40039> ;
        reg:hasSubproperty        <http://rdaregistry.info/Elements/i/P40045> ;
        reg:hasUnconstrained      <http://rdaregistry.info/Elements/u/P60297> ;
        rdfs:label                "est une reproduction de (item)"@fr ;
        skos:definition           "Met un item en relation avec un item qui sert de base à une reproduction."@fr ;
        rdakit:toolkitLabel       "reproduction de (item)"@fr ;
        rdakit:toolkitDefinition  "Item qui sert de base à une reproduction."@fr ;
        rdakit:toolkitLabel       "reproducción de (ítem)"@es ;
        rdakit:toolkitDefinition  "Un ítem que es usado como base para una reproducción."@es ;
        rdakit:instructionNumber  "24.5" ;
        reg:hasSubproperty        <http://rdaregistry.info/Elements/i/object/P40042> ;
        reg:name                  "saoChépCủaBản"@vi ;
        rdfs:label                "là sao chép của (bản)"@vi ;
        skos:definition           "Liên kết bản với bản được sử dụng như là cơ sở cho sản xuất lại."@vi ;
        rdakit:toolkitLabel       "sao chép của (bản)"@vi ;
        rdakit:toolkitDefinition  "Bản được sử dụng như là cơ sở cho sản xuất lại."@vi ;
        reg:name                  "reproduktionAfEksemplar"@da ;
        rdfs:label                "er reproduktion af (eksemplar)"@da ;
        reg:lexicalAlias          <http://rdaregistry.info/Elements/i/reproduktionAfEksemplar.da> ;
        skos:definition           "Relaterer et eksemplar til et eksemplar, der er anvendt som grundlag for en reproduktion."@da ;
        rdakit:toolkitLabel       "reproduktion af (eksemplar)"@da ;
        rdakit:toolkitDefinition  "Eksemplar, der er anvendt som grundlag for en reproduktion."@da ;
        rdfs:label                "ist Reproduktion von (Exemplar)"@de ;
        skos:definition           "Setzt ein Exemplar mit einem Exemplar, das als Grundlage für eine Reproduktion verwendet wurde, in Beziehung."@de ;
        rdakit:toolkitLabel       "Reproduktion von (Exemplar)"@de ;
        rdakit:toolkitDefinition  "Ein Exemplar, das als Grundlage für eine Reproduktion verwendet wurde."@de ;
        reg:name                  "αναπαραγωγήΤουΑντιτύπου"@el ;
        rdfs:label                "είναι αναπαραγωγή του (αντίτυπο)"@el ;
        reg:lexicalAlias          <http://rdaregistry.info/Elements/i/αναπαραγωγήΤουΑντιτύπου.el> ;
        skos:definition           "Συνδέει ένα αντίτυπο με ένα αντίτυπο το οποίο χρησιμοποιείται ως η βάση για μια αναπαραγωγή."@el ;
        rdakit:toolkitLabel       "αναπαραγωγή του (αντίτυπο)"@el ;
        rdakit:toolkitDefinition  "Ένα αντίτυπο το οποίο χρησιμοποιείται ως η βάση για μια αναπαραγωγή."@el ;
        rdfs:label                "és reproducció de (ítem)"@ca ;
        skos:definition           "Relaciona un item amb un ítem que s’usa com a base d’una reproducció."@ca ;
        rdakit:toolkitLabel       "reproducció de (ítem)"@ca ;
        rdakit:toolkitDefinition  "Ítem que s’usa com a base d’una reproducció."@ca ;
        reg:name                  "jaljenneKappaleesta"@fi ;
        rdfs:label                "jäljenne kappaleesta"@fi ;
        reg:lexicalAlias          <rdaa:jaljenneKappaleesta.fi> ;
        skos:definition           "Liittää kappaleen jäljentämisen perustana käytettyyn kappaleeseen."@fi ;
        rdakit:toolkitLabel       "jäljenne kappaleesta"@fi ;
        rdakit:toolkitDefinition  "Jäljentämisen perustana käytetty kappale."@fi ;
        reg:name                  "reproductionDeItem"@fr ;
        reg:lexicalAlias          <http://rdaregistry.info/Elements/i/reproductionDeItem.fr> ;
        rdakit:toolkitLabel       "reproduksjon av (eksemplar)"@no ;
        rdakit:toolkitDefinition  "Et eksemplar som brukes som utgangspunkt for en reproduksjon."@no ;
        reg:hasSubproperty        <http://rdaregistry.info/Elements/i/datatype/P40042> .

<http://rdaregistry.info/Elements/i/P40024>
        rdfs:isDefinedBy          <http://rdaregistry.info/Elements/i/> ;
        reg:status                <http://metadataregistry.org/uri/RegStatus/1001> ;
        reg:name                  "restorationistAgentOfItem"@en ;
        rdfs:label                "has restorationist agent of item"@en ;
        skos:definition           "Relates an item to an agent who is responsible for the set of technical, editorial, and intellectual procedures aimed at compensating for the degradation of an item by bringing it back to a state as close as possible to its original condition."@en ;
        rdf:type                  rdf:Property ;
        rdfs:domain               <http://rdaregistry.info/Elements/c/C10003> ;
        rdfs:subPropertyOf        <http://rdaregistry.info/Elements/i/P40093> ;
        reg:lexicalAlias          <http://rdaregistry.info/Elements/i/restorationistAgentOfItem.en> ;
        reg:hasUnconstrained      <http://rdaregistry.info/Elements/u/P60450> ;
        rdakit:toolkitLabel       "restorationist agent of item"@en ;
        rdakit:toolkitDefinition  "An agent who is responsible for the set of technical, editorial, and intellectual procedures aimed at compensating for the degradation of an item by bringing it back to a state as close as possible to its original condition."@en ;
        rdfs:label                "a pour agent restaurateur d’un item"@fr ;
        skos:definition           "Met un item en relation avec un agent qui est responsable de l’ensemble des procédures techniques, éditoriales et intellectuelles destinées à compenser la dégradation d’un item en le ramenant à un état aussi près que possible de sa condition originelle."@fr ;
        rdakit:toolkitLabel       "agent restaurateur d’un item"@fr ;
        rdakit:toolkitDefinition  "Agent qui est responsable de l’ensemble des procédures techniques, éditoriales et intellectuelles destinées à compenser la dégradation d’un item en le ramenant à un état aussi près que possible de sa condition originelle."@fr ;
        rdakit:toolkitLabel       "restaurador"@es ;
        rdakit:toolkitDefinition  "Una persona, familia o entidad corporativa responsable del conjunto de procedimientos técnicos, editoriales e intelectuales orientados a compensar la degradación de un ítem devolviéndolo a un estado lo más cercano posible a su estado original."@es ;
        rdakit:instructionNumber  "18.5" ;
        reg:hasSubproperty        <http://rdaregistry.info/Elements/i/object/P40024> ;
        reg:name                  "bảnNgườiPhụcChế"@vi ;
        rdfs:label                "có người phục chế (bản)"@vi ;
        skos:definition           "Liên kết bản với tác nhân có trách nhiệm tới chuỗi các quy trình kỹ thuật, biên tập, và trí tuệ trong việc khắc phục sự xuống cấp của bản bằng cách đưa nó về trạng thái gần giống nhất có thể với điều kiện nguyên gốc."@vi ;
        rdakit:toolkitLabel       "người phục chế (bản)"@vi ;
        rdakit:toolkitDefinition  "Tác nhân có trách nhiệm tới chuỗi các quy trình kỹ thuật, biên tập, và trí tuệ trong việc khắc phục sự xuống cấp của bản bằng cách đưa nó về trạng thái gần giống nhất có thể với điều kiện nguyên gốc."@vi ;
        reg:name                  "konservatorEksemplar"@da ;
        rdfs:label                "har konservator (eksemplar)"@da ;
        reg:lexicalAlias          <http://rdaregistry.info/Elements/i/konservatorEksemplar.da> ;
        skos:definition           "Relaterer et eksemplar til en agent, der er ansvarlig for rækken af tekniske, redaktionsmæssige og intellektuelle procedurer, der sigter mod at kompensere for forringelsen af et eksemplar ved at føre det tilbage til en tilstand, der er så tæt som muligt på dets oprindelige tilstand."@da ;
        rdakit:toolkitLabel       "konservator (eksemplar)"@da ;
        rdakit:toolkitDefinition  "Agent, der er ansvarlig for rækken af tekniske, redaktionsmæssige og intellektuelle procedurer, der sigter mod at kompensere for forringelsen af et eksemplar ved at føre det tilbage til en tilstand, der er så tæt som muligt på dets oprindelige tilstand."@da ;
        rdfs:label                "hat Restaurator (Exemplar)"@de ;
        skos:definition           "Setzt ein Exemplar mit einem Akteur, der an einer Expression eines Werks mitwirkt, indem er durch die Wiederherstellung und/oder Zusammenführung früherer Expressionen, die beschädigt oder unvollständig sein können, eine neue Expression erstellt, in Beziehung."@de ;
        rdakit:toolkitLabel       "Restaurator (Exemplar)"@de ;
        rdakit:toolkitDefinition  "Ein Akteur, der an einer Expression eines Werks mitwirkt, indem er durch die Wiederherstellung und/oder Zusammenführung früherer Expressionen, die beschädigt oder unvollständig sein können, eine neue Expression erstellt."@de ;
        reg:name                  "συντηρητήςΑντιτύπου"@el ;
        rdfs:label                "έχει συντηρητή (αντίτυπο)"@el ;
        reg:lexicalAlias          <http://rdaregistry.info/Elements/i/συντηρητήςΑντιτύπου.el> ;
        skos:definition           "Συνδέει ένα αντίτυπο με έναν φορέα υπεύθυνο για το σύνολο των τεχνικών, συντακτικών και διανοητικών διαδικασιών που στοχεύουν στην αποκατάσταση της αποδόμησης ενός αντιτύπου επαναφέροντάς το όσο το δυνατόν εγγύτερα στην αρχική του κατάσταση."@el ;
        rdakit:toolkitLabel       "συντηρητής (αντίτυπο)"@el ;
        rdakit:toolkitDefinition  "Ένας φορέας υπεύθυνος για το σύνολο των τεχνικών, συντακτικών και διανοητικών διαδικασιών που στοχεύουν στην αποκατάσταση της αποδόμησης ενός αντιτύπου επαναφέροντάς το όσο το δυνατόν εγγύτερα στην αρχική του κατάσταση."@el ;
        rdfs:label                "té com a restaurador (ítem)"@ca ;
        skos:definition           "Relaciona un item amb un agent responsable del conjunt de procediments tècnics, editorials i intel·lectuals destinats a compensar la degradació d’un ítem retornant-lo a un estat que s’aproximi al màxim a la seva condició original"@ca ;
        rdakit:toolkitLabel       "restaurador (ítem)"@ca ;
        rdakit:toolkitDefinition  "Agent responsable del conjunt de procediments tècnics, editorials i intel·lectuals destinats a compensar la degradació d’un ítem retornant-lo a un estat que s’aproximi al màxim a la seva condició original."@ca ;
        reg:name                  "entisoijaKappale"@fi ;
        rdfs:label                "entisöijä (kappale)"@fi ;
        reg:lexicalAlias          <rdaa:entisoijaKappale.fi> ;
        skos:definition           "Liittää kappaleen toimijaan, joka vastaa teknisistä, toimituksellisista ja tiedollisista toimenpiteistä, joiden tarkoitus on palauttaa kappale mahdollisimman lähelle sen alkuperäistä tilaa tai kuntoa."@fi ;
        rdakit:toolkitLabel       "entisöijä (kappale)"@fi ;
        rdakit:toolkitDefinition  "Toimija, joka vastaa teknisistä, toimituksellisista ja tiedollisista toimenpiteistä, joiden tarkoitus on palauttaa kappale mahdollisimman lähelle sen alkuperäistä tilaa tai kuntoa."@fi ;
        reg:name                  "restaurateurItem"@fr ;
        reg:lexicalAlias          <http://rdaregistry.info/Elements/i/agentRestaurateurDunItem.fr> ;
        rdakit:toolkitLabel       "konservator (eksemplar)"@no ;
        rdakit:toolkitDefinition  "En agent med ansvar for de tekniske og intellektuelle metodene som brukes for å kompensere for nedbrytningen av et eksemplar ved å restaurere det til en tilstand som er så lik originaltilstanden som mulig."@no ;
        rdakit:hasElementType     "2" ;
        reg:name                  "restaurátorPéldány"@hu ;
        rdfs:label                "van restaurátora (példány)"@hu ;
        skos:definition           "Egy példányt hozzákapcsol egy ágenshez (személyhez, családhoz vagy testülethez), aki/amely felelős egy sor technikai, szerkesztési és szellemi eljárásért, amelynek célja egy példány tönkremenetelének az ellensúlyozása oly módon, hogy azt az eredeti állapothoz lehető legközelebbi állapotba állítja vissza. "@hu ;
        rdakit:toolkitLabel       "restaurátor (példány)"@hu ;
        rdakit:toolkitDefinition  "Egy ágens (személy, család vagy testület), aki/amely felelős a technikai, szerkesztési és szellemi eljárásokért, amelyek célja egy példány leromlásának ellensúlyozása oly módon, hogy azt az eredeti állapothoz a lehető legközelebbi állapotba hozza vissza. "@hu ;
        reg:hasSubproperty        <http://rdaregistry.info/Elements/i/datatype/P40024> ;
        skos:altLabel             "restorationist (item)"@en ;
        skos:altLabel             "restaurateur (item)"@fr .

<http://rdaregistry.info/Elements/i/P40127>
        rdfs:isDefinedBy          <http://rdaregistry.info/Elements/i/> ;
        reg:status                <http://metadataregistry.org/uri/RegStatus/1001> ;
        rdfs:label                "has restorationist collective agent of item"@en ;
        reg:lexicalAlias          <http://rdaregistry.info/Elements/i/restorationistCollectiveAgentOfItem.en> ;
        skos:definition           "Relates an item to a collective agent who is responsible for the set of technical, editorial, and intellectual procedures aimed at compensating for the degradation of an item by bringing it back to a state as close as possible to its original condition."@en ;
        rdakit:toolkitLabel       "restorationist collective agent of item"@en ;
        rdakit:toolkitDefinition  "A collective agent who is responsible for the set of technical, editorial, and intellectual procedures aimed at compensating for the degradation of an item by bringing it back to a state as close as possible to its original condition."@en ;
        rdf:type                  rdf:Property ;
        reg:name                  "restorationistCollectiveAgentOfItem" ;
        rdfs:domain               <http://rdaregistry.info/Elements/c/C10003> ;
        rdakit:hasElementType     "2" ;
        reg:hasSubproperty        <http://rdaregistry.info/Elements/i/datatype/P40127> ;
        reg:hasSubproperty        <http://rdaregistry.info/Elements/i/object/P40127> ;
        rdfs:subPropertyOf        <http://rdaregistry.info/Elements/i/P40128> ;
        rdfs:subPropertyOf        <http://rdaregistry.info/Elements/i/P40024> ;
        reg:hasSubproperty        <http://rdaregistry.info/Elements/i/P40143> ;
        reg:hasSubproperty        <http://rdaregistry.info/Elements/i/P40159> ;
        reg:hasUnconstrained      <http://rdaregistry.info/Elements/u/P60450> ;
        rdfs:label                "a pour agent collectif restaurateur d’un item"@fr ;
        skos:definition           "Met un item en relation avec un agent collectif qui est responsable de l’ensemble des procédures techniques, éditoriales et intellectuelles destinées à compenser la dégradation d’un item en le ramenant à un état aussi près que possible de sa condition originelle."@fr ;
        rdakit:toolkitLabel       "agent collectif restaurateur d’un item"@fr ;
        rdakit:toolkitDefinition  "Agent collectif qui est responsable de l’ensemble des procédures techniques, éditoriales et intellectuelles destinées à compenser la dégradation d’un item en le ramenant à un état aussi près que possible de sa condition originelle."@fr ;
        reg:lexicalAlias          <http://rdaregistry.info/Elements/i/agentCollectifRestaurateurDunItem.fr> .

<http://rdaregistry.info/Elements/i/P40143>
        rdfs:isDefinedBy          <http://rdaregistry.info/Elements/i/> ;
        reg:status                <http://metadataregistry.org/uri/RegStatus/1001> ;
        rdfs:label                "has restorationist corporate body of item"@en ;
        reg:lexicalAlias          <http://rdaregistry.info/Elements/i/restorationistCorporateBodyOfItem.en> ;
        skos:definition           "Relates an item to a corporate body who is responsible for the set of technical, editorial, and intellectual procedures aimed at compensating for the degradation of an item by bringing it back to a state as close as possible to its original condition."@en ;
        rdakit:toolkitLabel       "restorationist corporate body of item"@en ;
        rdakit:toolkitDefinition  "A corporate body who is responsible for the set of technical, editorial, and intellectual procedures aimed at compensating for the degradation of an item by bringing it back to a state as close as possible to its original condition."@en ;
        rdf:type                  rdf:Property ;
        reg:name                  "restorationistCorporateBodyOfItem" ;
        rdfs:domain               <http://rdaregistry.info/Elements/c/C10003> ;
        rdakit:hasElementType     "2" ;
        reg:hasSubproperty        <http://rdaregistry.info/Elements/i/datatype/P40143> ;
        reg:hasSubproperty        <http://rdaregistry.info/Elements/i/object/P40143> ;
        rdfs:subPropertyOf        <http://rdaregistry.info/Elements/i/P40144> ;
        rdfs:subPropertyOf        <http://rdaregistry.info/Elements/i/P40127> ;
        reg:hasUnconstrained      <http://rdaregistry.info/Elements/u/P60450> ;
        rdfs:label                "a pour collectivité restauratrice d’un item"@fr ;
        skos:definition           "Met un item en relation avec une collectivité qui est responsable de l’ensemble des procédures techniques, éditoriales et intellectuelles destinées à compenser la dégradation d’un item en le ramenant à un état aussi près que possible de sa condition originelle."@fr ;
        rdakit:toolkitLabel       "collectivité restauratrice d’un item"@fr ;
        rdakit:toolkitDefinition  "Collectivité qui est responsable de l’ensemble des procédures techniques, éditoriales et intellectuelles destinées à compenser la dégradation d’un item en le ramenant à un état aussi près que possible de sa condition originelle."@fr ;
        reg:lexicalAlias          <http://rdaregistry.info/Elements/i/collectivitéRestauratriceDunItem.fr> .

<http://rdaregistry.info/Elements/i/P40159>
        rdfs:isDefinedBy          <http://rdaregistry.info/Elements/i/> ;
        reg:status                <http://metadataregistry.org/uri/RegStatus/1001> ;
        rdfs:label                "has restorationist family of item"@en ;
        reg:lexicalAlias          <http://rdaregistry.info/Elements/i/restorationistFamilyOfItem.en> ;
        skos:definition           "Relates an item to a family who is responsible for the set of technical, editorial, and intellectual procedures aimed at compensating for the degradation of an item by bringing it back to a state as close as possible to its original condition."@en ;
        rdakit:toolkitLabel       "restorationist family of item"@en ;
        rdakit:toolkitDefinition  "A family who is responsible for the set of technical, editorial, and intellectual procedures aimed at compensating for the degradation of an item by bringing it back to a state as close as possible to its original condition."@en ;
        rdf:type                  rdf:Property ;
        reg:name                  "restorationistFamilyOfItem" ;
        rdfs:domain               <http://rdaregistry.info/Elements/c/C10003> ;
        rdakit:hasElementType     "2" ;
        reg:hasSubproperty        <http://rdaregistry.info/Elements/i/datatype/P40159> ;
        reg:hasSubproperty        <http://rdaregistry.info/Elements/i/object/P40159> ;
        rdfs:subPropertyOf        <http://rdaregistry.info/Elements/i/P40160> ;
        rdfs:subPropertyOf        <http://rdaregistry.info/Elements/i/P40127> ;
        reg:hasUnconstrained      <http://rdaregistry.info/Elements/u/P60450> ;
        rdfs:label                "a pour famille restauratrice d’un item"@fr ;
        skos:definition           "Met un item en relation avec une famille qui est responsable de l’ensemble des procédures techniques, éditoriales et intellectuelles destinées à compenser la dégradation d’un item en le ramenant à un état aussi près que possible de sa condition originelle."@fr ;
        rdakit:toolkitLabel       "famille restauratrice d’un item"@fr ;
        rdakit:toolkitDefinition  "Famille qui est responsable de l’ensemble des procédures techniques, éditoriales et intellectuelles destinées à compenser la dégradation d’un item en le ramenant à un état aussi près que possible de sa condition originelle."@fr ;
        reg:lexicalAlias          <http://rdaregistry.info/Elements/i/familleRestauratriceDunItem.fr> .

<http://rdaregistry.info/Elements/i/P40111>
        rdfs:isDefinedBy          <http://rdaregistry.info/Elements/i/> ;
        reg:status                <http://metadataregistry.org/uri/RegStatus/1001> ;
        rdfs:label                "has restorationist person of item"@en ;
        reg:lexicalAlias          <http://rdaregistry.info/Elements/i/restorationistPersonOfItem.en> ;
        skos:definition           "Relates an item to a person who is responsible for the set of technical, editorial, and intellectual procedures aimed at compensating for the degradation of an item by bringing it back to a state as close as possible to its original condition."@en ;
        rdakit:toolkitLabel       "restorationist person of item"@en ;
        rdakit:toolkitDefinition  "A person who is responsible for the set of technical, editorial, and intellectual procedures aimed at compensating for the degradation of an item by bringing it back to a state as close as possible to its original condition."@en ;
        rdf:type                  rdf:Property ;
        reg:name                  "restorationistPersonOfItem" ;
        rdfs:domain               <http://rdaregistry.info/Elements/c/C10003> ;
        rdakit:hasElementType     "2" ;
        reg:hasSubproperty        <http://rdaregistry.info/Elements/i/datatype/P40111> ;
        reg:hasSubproperty        <http://rdaregistry.info/Elements/i/object/P40111> ;
        rdfs:subPropertyOf        <http://rdaregistry.info/Elements/i/P40112> ;
        rdfs:subPropertyOf        <http://rdaregistry.info/Elements/i/P40024> ;
        reg:hasUnconstrained      <http://rdaregistry.info/Elements/u/P60450> ;
        rdfs:label                "a pour personne restauratrice d’un item"@fr ;
        skos:definition           "Met un item en relation avec une personne qui est responsable de l’ensemble des procédures techniques, éditoriales et intellectuelles destinées à compenser la dégradation d’un item en le ramenant à un état aussi près que possible de sa condition originelle."@fr ;
        rdakit:toolkitLabel       "personne restauratrice d’un item"@fr ;
        rdakit:toolkitDefinition  "Personne qui est responsable de l’ensemble des procédures techniques, éditoriales et intellectuelles destinées à compenser la dégradation d’un item en le ramenant à un état aussi près que possible de sa condition originelle."@fr ;
        reg:lexicalAlias          <http://rdaregistry.info/Elements/i/personneRestauratriceDunItem.fr> .

<http://rdaregistry.info/Elements/i/P40047>
        rdfs:isDefinedBy          <http://rdaregistry.info/Elements/i/> ;
        reg:status                <http://metadataregistry.org/uri/RegStatus/1001> ;
        reg:name                  "restrictionOnAccessToItem"@en ;
        rdfs:label                "has restriction on access to item"@en ;
        skos:definition           "Relates an item to a limitation placed on access to an item."@en ;
        rdf:type                  rdf:Property ;
        rdfs:domain               <http://rdaregistry.info/Elements/c/C10003> ;
        reg:lexicalAlias          <http://rdaregistry.info/Elements/i/restrictionOnAccessToItem.en> ;
        reg:hasUnconstrained      <http://rdaregistry.info/Elements/u/P60496> ;
        rdakit:instructionNumber  "4.4" ;
        rdakit:toolkitLabel       "restriction on access to item"@en ;
        rdakit:toolkitDefinition  "A limitation placed on access to an item."@en ;
        rdfs:label                "a pour restriction d’accès à un item"@fr ;
        skos:definition           "Met un item en relation avec une limitation imposée sur l’accès à un item."@fr ;
        rdakit:toolkitLabel       "restriction d’accès à un item"@fr ;
        rdakit:toolkitDefinition  "Limitation imposée sur l’accès à un item."@fr ;
        rdakit:toolkitLabel       "restricciones de acceso"@es ;
        rdakit:toolkitDefinition  "Limitaciones establecidas para el acceso a un recurso."@es ;
        reg:hasSubproperty        <http://rdaregistry.info/Elements/i/object/P40047> ;
        rdfs:label                "har åtkomstrestriktioner"@sv ;
        rdakit:toolkitLabel       "åtkomstrestriktioner"@sv ;
        reg:name                  "cấmTruyCậpVàoBản"@vi ;
        rdfs:label                "có cấm truy cập vào bản"@vi ;
        skos:definition           "Liên kết bản với giới hạn được đặt ra về truy cấp tới bản."@vi ;
        rdakit:toolkitLabel       "cấm truy cập vào bản"@vi ;
        rdakit:toolkitDefinition  "Giới hạn được đặt ra về truy cấp tới bản."@vi ;
        reg:name                  "adgangsrestriktionerTilEksemplar"@da ;
        rdfs:label                "har adgangsrestriktioner til eksemplar"@da ;
        reg:lexicalAlias          <http://rdaregistry.info/Elements/i/adgangsrestriktionerTilEksemplar.da> ;
        skos:definition           "Relaterer et eksemplar til bgrænsninger for adgang til et eksemplar."@da ;
        rdakit:toolkitLabel       "adgangsrestriktioner til eksemplar"@da ;
        rdakit:toolkitDefinition  "Begrænsninger for adgang til et eksemplar."@da ;
        rdfs:label                "hat Zugangsbeschränkung zu einem Exemplar"@de ;
        skos:definition           "Setzt ein Exemplar mit einer Beschränkung des Zugangs zu einem Exemplar in Beziehung."@de ;
        rdakit:toolkitLabel       "Zugangsbeschränkung zu einem Exemplar"@de ;
        rdakit:toolkitDefinition  "Eine Beschränkung des Zugangs zu einem Exemplar"@de ;
        reg:name                  "περιορισμόςΣτηνΠρόσβασηΣτοΑντίτυπο"@el ;
        rdfs:label                "έχει περιορισμό στην πρόσβαση στο αντίτυπο"@el ;
        reg:lexicalAlias          <http://rdaregistry.info/Elements/i/περιορισμόςΣτηνΠρόσβασηΣτοΑντίτυπο.el> ;
        skos:definition           "Συνδέει ένα αντίτυπο με έναν περιορισμό που ανατίθεται στην πρόσβαση σε ένα αντίτυπο."@el ;
        rdakit:toolkitLabel       "περιορισμός στην πρόσβαση στο αντίτυπο"@el ;
        rdakit:toolkitDefinition  "Ένας περιορισμός που ανατίθεται στην πρόσβαση σε ένα αντίτυπο."@el ;
        rdfs:label                "té com a restriccions d’accés a un ítem"@ca ;
        skos:definition           "Relaciona un item amb les limitacions imposades sobre l’accés a un ítem."@ca ;
        rdakit:toolkitLabel       "restriccions d’accés a un ítem"@ca ;
        rdakit:toolkitDefinition  "Limitacions imposades sobre l’accés a un ítem."@ca ;
        reg:name                  "kappaleenSaatavuudenRajoitukset"@fi ;
        rdfs:label                "kappaleen saatavuuden rajoitukset"@fi ;
        reg:lexicalAlias          <rdaa:kappaleenSaatavuudenRajoitukset.fi> ;
        skos:definition           "Liittää kappaleen kappaleen saatavuudelle asetettuihin rajoituksiin."@fi ;
        rdakit:toolkitLabel       "kappaleen saatavuuden rajoitukset"@fi ;
        rdakit:toolkitDefinition  "Kappaleen käyttöön saamiselle asetettuja rajoituksia."@fi ;
        reg:name                  "restrictionDaccèsÀUnItem"@fr ;
        reg:lexicalAlias          <http://rdaregistry.info/Elements/i/restrictionDaccèsÀUnItem.fr> ;
        rdakit:toolkitLabel       "adgangsbegrensning for eksemplar"@no ;
        rdakit:toolkitDefinition  "En begrensning for tilgangen til en ressurs."@no ;
        rdakit:hasElementType     "6" ;
        reg:name                  "Példányhozzáféréskorlátozása"@hu ;
        rdfs:label                "van példányhozzáférési korlátozása"@hu ;
        skos:definition           "Egy példányt hozzákapcsol egy korlátozáshoz, amelyet egy példány hozzáférésére állítottak."@hu ;
        rdakit:toolkitLabel       "hozzáférési korlátozás példányhoz"@hu ;
        rdakit:toolkitDefinition  "Egy példány hozzáféréséhez kapcsolt korlátozás."@hu ;
        reg:hasSubproperty        <http://rdaregistry.info/Elements/i/datatype/P40047> .

<http://rdaregistry.info/Elements/i/P40048>
        rdfs:isDefinedBy          <http://rdaregistry.info/Elements/i/> ;
        reg:status                <http://metadataregistry.org/uri/RegStatus/1001> ;
        reg:name                  "restrictionOnUseOfItem"@en ;
        rdfs:label                "has restriction on use of item"@en ;
        skos:definition           "Relates an item to a limitation placed on reproduction, publication, exhibition, etc., of an item."@en ;
        rdf:type                  rdf:Property ;
        rdfs:domain               <http://rdaregistry.info/Elements/c/C10003> ;
        reg:lexicalAlias          <http://rdaregistry.info/Elements/i/restrictionOnUseOfItem.en> ;
        reg:hasUnconstrained      <http://rdaregistry.info/Elements/u/P60497> ;
        rdakit:instructionNumber  "4.5" ;
        rdakit:toolkitLabel       "restriction on use of item"@en ;
        rdakit:toolkitDefinition  "A limitation placed on reproduction, publication, exhibition, etc., of an item."@en ;
        rdfs:label                "a pour restriction d’usage d’un item"@fr ;
        skos:definition           "Met un item en relation avec une limitation imposée sur la reproduction, la publication, l’exposition, etc. d’un item."@fr ;
        rdakit:toolkitLabel       "restriction d’usage d’un item"@fr ;
        rdakit:toolkitDefinition  "Limitation imposée sur la reproduction, la publication, l’exposition, etc. d’un item."@fr ;
        rdakit:toolkitLabel       "restricciones sobre el uso"@es ;
        rdakit:toolkitDefinition  "Limitaciones establecidas sobre los usos, tales como reproducción, publicación, exhibición, etc."@es ;
        reg:hasSubproperty        <http://rdaregistry.info/Elements/i/object/P40048> ;
        rdfs:label                "har användningsrestriktioner"@sv ;
        rdakit:toolkitLabel       "användningsrestriktioner"@sv ;
        reg:name                  "cấmSửDụngBản"@vi ;
        rdfs:label                "có cấm sử dụng bản"@vi ;
        skos:definition           "Liên kết bản với giới hạn được đặt ra về sản xuất lại, xuất bản, triển lãm, v.v..., của bản."@vi ;
        rdakit:toolkitLabel       "cấm sử dụng bản"@vi ;
        rdakit:toolkitDefinition  "Giới hạn được đặt ra về sản xuất lại, xuất bản, triển lãm, v.v..., của bản."@vi ;
        reg:name                  "brugsrestriktionerForEksemplar"@da ;
        rdfs:label                "har brugsgrestriktioner for eksemplar"@da ;
        reg:lexicalAlias          <http://rdaregistry.info/Elements/i/brugsrestriktionerForEksemplar.da> ;
        skos:definition           "Relaterer et eksemplar til begrænsninger vedr. ret til reproduktion, publicering, udstilling etc."@da ;
        rdakit:toolkitLabel       "brugsrestriktioner for eksemplar"@da ;
        rdakit:toolkitDefinition  "Begrænsninger vedr. ret til reproduktion, publicering, udstilling etc."@da ;
        rdfs:label                "hat Benutzungsbeschränkung für ein Exemplar"@de ;
        skos:definition           "Setzt ein Exemplar mit einer Beschränkung für die Reproduktion, Veröffentlichung, Ausstellung usw. eines Exemplars, in Beziehung."@de ;
        rdakit:toolkitLabel       "Benutzungsbeschränkung für ein Exemplar"@de ;
        rdakit:toolkitDefinition  "Eine Beschränkung für die Reproduktion, Veröffentlichung, Ausstellung usw. eines Exemplars."@de ;
        reg:name                  "περιορισμόςΣτηΧρήσηΤουΑντιτύπου"@el ;
        rdfs:label                "έχει περιορισμό στη χρήση του αντιτύπου"@el ;
        reg:lexicalAlias          <http://rdaregistry.info/Elements/i/περιορισμόςΣτηΧρήσηΤουΑντιτύπου.el> ;
        skos:definition           "Συνδέει ένα αντίτυπο με έναν περιορισμό που ανατίθεται στην αναπαραγωγή, τη δημοσίευση, την έκθεση κ.λπ. ενός αντιτύπου."@el ;
        rdakit:toolkitLabel       "περιορισμός στη χρήση του αντιτύπου"@el ;
        rdakit:toolkitDefinition  "Ένας περιορισμός που ανατίθεται στην αναπαραγωγή, τη δημοσίευση, την έκθεση κ.λπ. ενός αντιτύπου."@el ;
        rdfs:label                "té com a restriccions d’ús d’un ítem"@ca ;
        skos:definition           "Relaciona un item amb les limitacions imposades sobre usos d’un ítem, com ara la reproducció, la publicació, l’exposició, etc."@ca ;
        rdakit:toolkitLabel       "restriccions d’ús d’un ítem"@ca ;
        rdakit:toolkitDefinition  "Limitacions imposades sobre usos d’un ítem, com ara la reproducció, la publicació, l’exposició, etc."@ca ;
        reg:name                  "kappaleenKayttoehdot"@fi ;
        rdfs:label                "kappaleen käyttöehdot"@fi ;
        reg:lexicalAlias          <rdaa:kappaleenKayttoehdot.fi> ;
        skos:definition           "Liittää kappaleen kappaleen käyttöä koskeviin rajoituksiin, esim. kopiointia, julkaisemista tai esille asettamista."@fi ;
        rdakit:toolkitLabel       "kappaleen käyttöehdot"@fi ;
        rdakit:toolkitDefinition  "Rajoituksia, jotka koskevat kappaleen käyttöä, esim. kopiointia, julkaisua tai esille asettamista."@fi ;
        reg:name                  "restrictionDusageDunItem"@fr ;
        reg:lexicalAlias          <http://rdaregistry.info/Elements/i/restrictionDusageDunItem.fr> ;
        rdakit:toolkitLabel       "restriksjoner for bruk av eksemplar"@no ;
        rdakit:toolkitDefinition  "En begrensning for reproduksjon, utgivelse, utstilling etc. av en ressurs."@no ;
        rdakit:hasElementType     "6" ;
        reg:name                  "Példányhasználatkorlátozása"@hu ;
        rdfs:label                "van példányhasználati korlátozása"@hu ;
        skos:definition           "Egy példányt hozzákapcsol egy korlátozáshoz, amelyet egy példány másolására, kiadására, kiállítására stb. állítottak."@hu ;
        rdakit:toolkitLabel       "használati korlátozás példányhoz"@hu ;
        rdakit:toolkitDefinition  "Egy példány reprodukciójához, kiadásához, kiállításához stb. kapcsolt korlátozás."@hu ;
        reg:hasSubproperty        <http://rdaregistry.info/Elements/i/datatype/P40048> .

<http://rdaregistry.info/Elements/i/P40040>
        rdfs:isDefinedBy    <http://rdaregistry.info/Elements/i/> ;
        reg:status          <http://metadataregistry.org/uri/RegStatus/1008> ;
        rdf:type            rdf:Property ;
        rdfs:subPropertyOf  <http://rdaregistry.info/Elements/i/P40030> .

<http://rdaregistry.info/Elements/i/P40008>
        rdfs:isDefinedBy          <http://rdaregistry.info/Elements/i/> ;
        reg:status                <http://metadataregistry.org/uri/RegStatus/1001> ;
        reg:name                  "sellerAgent"@en ;
        rdfs:label                "has seller agent"@en ;
        skos:definition           "Relates an item to an agent who is a former owner of an item who sells the item to another owner."@en ;
        rdf:type                  rdf:Property ;
        rdfs:domain               <http://rdaregistry.info/Elements/c/C10003> ;
        rdfs:subPropertyOf        <http://rdaregistry.info/Elements/i/P40019> ;
        reg:lexicalAlias          <http://rdaregistry.info/Elements/i/sellerAgent.en> ;
        reg:hasUnconstrained      <http://rdaregistry.info/Elements/u/P60092> ;
        rdakit:toolkitLabel       "seller agent"@en ;
        rdakit:toolkitDefinition  "An agent who is a former owner of an item who sells the item to another owner."@en ;
        rdfs:label                "a pour agent vendeur"@fr ;
        skos:definition           "Met un item en relation avec un ancien agent propriétaire d’un item qui a vendu cet item à un autre propriétaire."@fr ;
        rdakit:toolkitLabel       "agent vendeur"@fr ;
        rdakit:toolkitDefinition  "Ancien agent propriétaire d’un item qui a vendu cet item à un autre propriétaire."@fr ;
        rdakit:toolkitLabel       "vendedor"@es ;
        rdakit:toolkitDefinition  "Un propietario anterior de un ítem que lo vendió a otro propietario."@es ;
        rdakit:instructionNumber  "18.5" ;
        reg:hasSubproperty        <http://rdaregistry.info/Elements/i/object/P40008> ;
        reg:name                  "ngườiBán"@vi ;
        rdfs:label                "có người bán"@vi ;
        skos:definition           "Liên kết bản với người chủ trước đây của bản, người đã bán bản đó cho người chủ khác."@vi ;
        rdakit:toolkitLabel       "người bán"@vi ;
        rdakit:toolkitDefinition  "Người chủ trước đây của bản, người đã bán bản đó cho người chủ khác."@vi ;
        reg:name                  "sælger"@da ;
        rdfs:label                "har sælger"@da ;
        reg:lexicalAlias          <http://rdaregistry.info/Elements/i/sælger.da> ;
        skos:definition           "Relaterer et eksemplar til en tidligere ejer af et eksemplar, der har solgt dette eksemplar til en anden ejer."@da ;
        rdakit:toolkitLabel       "sælger"@da ;
        rdakit:toolkitDefinition  "Tidligere ejer af et eksemplar, der har solgt dette eksemplar til en anden ejer."@da ;
        rdfs:label                "hat Verkäufer"@de ;
        skos:definition           "Setzt ein Exemplar mit einem früheren Eigentümer eines Exemplars, der dieses Exemplar an einen anderen Eigentümer verkauft hat, in Beziehung."@de ;
        rdakit:toolkitLabel       "Verkäufer"@de ;
        rdakit:toolkitDefinition  "Ein früherer Eigentümer eines Exemplars, der dieses Exemplar an einen anderen Eigentümer verkauft hat."@de ;
        reg:name                  "πωλητής"@el ;
        rdfs:label                "έχει πωλητή"@el ;
        reg:lexicalAlias          <http://rdaregistry.info/Elements/i/πωλητής.el> ;
        skos:definition           "Συνδέει ένα αντίτυπο με έναν προηγούμενο ιδιοκτήτη ενός αντιτύπου ο οποίος πούλησε αυτό το αντίτυπο σε κάποιον άλλον ιδιοκτήτη."@el ;
        rdakit:toolkitLabel       "πωλητής"@el ;
        rdakit:toolkitDefinition  "Ένας προηγούμενος ιδιοκτήτης ενός αντιτύπου, ο οποίος πούλησε αυτό το αντίτυπο σε κάποιον άλλον ιδιοκτήτη."@el ;
        rdfs:label                "té com a venedor"@ca ;
        skos:definition           "Relaciona un item amb un propietari anterior d’un ítem que el va vendre a un altre propietari."@ca ;
        rdakit:toolkitLabel       "venedor"@ca ;
        rdakit:toolkitDefinition  "Propietari anterior d’un ítem que el va vendre a un altre propietari."@ca ;
        reg:name                  "myyja"@fi ;
        rdfs:label                "myyjä"@fi ;
        reg:lexicalAlias          <rdaa:myyja.fi> ;
        skos:definition           "Liittää kappaleen sen aikaisempaan omistajaan, joka on myynyt sen toiselle omistajalle."@fi ;
        rdakit:toolkitLabel       "myyjä"@fi ;
        rdakit:toolkitDefinition  "Kappaleen aikaisempi omistaja, joka on myynyt sen toiselle omistajalle."@fi ;
        reg:name                  "vendeur"@fr ;
        reg:lexicalAlias          <http://rdaregistry.info/Elements/i/agentVendeur.fr> ;
        rdakit:toolkitLabel       "selger"@no ;
        rdakit:toolkitDefinition  "En tidligere eier av et eksemplar, som har solgt eksemplaret til en annen eier."@no ;
        rdakit:hasElementType     "2" ;
        reg:name                  "eladó"@hu ;
        rdfs:label                "van eladója"@hu ;
        skos:definition           "Egy példányt hozzákapcsol egy példány korábbi tulajdonosához, aki a tételt egy másik tulajdonosnak eladta."@hu ;
        rdakit:toolkitLabel       "eladó"@hu ;
        rdakit:toolkitDefinition  "Egy példány korábbi tulajdonosa, aki a példányt egy másik tulajdonosnak eladta."@hu ;
        skos:altLabel             "seller"@en ;
        skos:altLabel             "vendeur"@fr .

<http://rdaregistry.info/Elements/i/P40125>
        rdfs:isDefinedBy          <http://rdaregistry.info/Elements/i/> ;
        reg:status                <http://metadataregistry.org/uri/RegStatus/1001> ;
        rdfs:label                "has seller collective agent"@en ;
        reg:lexicalAlias          <http://rdaregistry.info/Elements/i/sellerCollectiveAgent.en> ;
        skos:definition           "Relates an item to a collective agent who is a former owner of an item who sells the item to another owner."@en ;
        rdakit:toolkitLabel       "seller collective agent"@en ;
        rdakit:toolkitDefinition  "A collective agent who is a former owner of an item who sells the item to another owner."@en ;
        rdf:type                  rdf:Property ;
        reg:name                  "sellerCollectiveAgent" ;
        rdfs:domain               <http://rdaregistry.info/Elements/c/C10003> ;
        rdakit:hasElementType     "2" ;
        reg:hasSubproperty        <http://rdaregistry.info/Elements/i/datatype/P40125> ;
        reg:hasSubproperty        <http://rdaregistry.info/Elements/i/object/P40125> ;
        rdfs:subPropertyOf        <http://rdaregistry.info/Elements/i/P40118> ;
        rdfs:subPropertyOf        <http://rdaregistry.info/Elements/i/P40008> ;
        reg:hasSubproperty        <http://rdaregistry.info/Elements/i/P40141> ;
        reg:hasSubproperty        <http://rdaregistry.info/Elements/i/P40157> ;
        reg:hasUnconstrained      <http://rdaregistry.info/Elements/u/P60092> ;
        rdfs:label                "a pour agent collectif vendeur"@fr ;
        skos:definition           "Met un item en relation avec un ancien agent collectif propriétaire d’un item qui a vendu cet item à un autre propriétaire."@fr ;
        rdakit:toolkitLabel       "agent collectif vendeur"@fr ;
        rdakit:toolkitDefinition  "Ancien agent collectif propriétaire d’un item qui a vendu cet item à un autre propriétaire."@fr ;
        reg:lexicalAlias          <http://rdaregistry.info/Elements/i/agentCollectifVendeur.fr> .

<http://rdaregistry.info/Elements/i/P40141>
        rdfs:isDefinedBy          <http://rdaregistry.info/Elements/i/> ;
        reg:status                <http://metadataregistry.org/uri/RegStatus/1001> ;
        rdfs:label                "has seller corporate body"@en ;
        reg:lexicalAlias          <http://rdaregistry.info/Elements/i/sellerCorporateBody.en> ;
        skos:definition           "Relates an item to a corporate body who is a former owner of an item who sells the item to another owner."@en ;
        rdakit:toolkitLabel       "seller corporate body"@en ;
        rdakit:toolkitDefinition  "A corporate body who is a former owner of an item who sells the item to another owner."@en ;
        rdf:type                  rdf:Property ;
        reg:name                  "sellerCorporateBody" ;
        rdfs:domain               <http://rdaregistry.info/Elements/c/C10003> ;
        rdakit:hasElementType     "2" ;
        reg:hasSubproperty        <http://rdaregistry.info/Elements/i/datatype/P40141> ;
        reg:hasSubproperty        <http://rdaregistry.info/Elements/i/object/P40141> ;
        rdfs:subPropertyOf        <http://rdaregistry.info/Elements/i/P40134> ;
        rdfs:subPropertyOf        <http://rdaregistry.info/Elements/i/P40125> ;
        reg:hasUnconstrained      <http://rdaregistry.info/Elements/u/P60092> ;
        rdfs:label                "a pour collectivité vendeuse"@fr ;
        skos:definition           "Met un item en relation avec une ancienne collectivité propriétaire d’un item qui a vendu cet item à un autre propriétaire."@fr ;
        rdakit:toolkitLabel       "collectivité vendeuse"@fr ;
        rdakit:toolkitDefinition  "Ancienne collectivité propriétaire d’un item qui a vendu cet item à un autre propriétaire."@fr ;
        reg:lexicalAlias          <http://rdaregistry.info/Elements/i/collectivitéVendeuse.fr> .

<http://rdaregistry.info/Elements/i/P40157>
        rdfs:isDefinedBy          <http://rdaregistry.info/Elements/i/> ;
        reg:status                <http://metadataregistry.org/uri/RegStatus/1001> ;
        rdfs:label                "has seller family"@en ;
        reg:lexicalAlias          <http://rdaregistry.info/Elements/i/sellerFamily.en> ;
        skos:definition           "Relates an item to a family who is a former owner of an item who sells the item to another owner."@en ;
        rdakit:toolkitLabel       "seller family"@en ;
        rdakit:toolkitDefinition  "A family who is a former owner of an item who sells the item to another owner."@en ;
        rdf:type                  rdf:Property ;
        reg:name                  "sellerFamily" ;
        rdfs:domain               <http://rdaregistry.info/Elements/c/C10003> ;
        rdakit:hasElementType     "2" ;
        reg:hasSubproperty        <http://rdaregistry.info/Elements/i/datatype/P40157> ;
        reg:hasSubproperty        <http://rdaregistry.info/Elements/i/object/P40157> ;
        rdfs:subPropertyOf        <http://rdaregistry.info/Elements/i/P40150> ;
        rdfs:subPropertyOf        <http://rdaregistry.info/Elements/i/P40125> ;
        reg:hasUnconstrained      <http://rdaregistry.info/Elements/u/P60092> ;
        rdfs:label                "a pour famille vendeuse"@fr ;
        skos:definition           "Met un item en relation avec une ancienne famille propriétaire d’un item qui a vendu cet item à un autre propriétaire."@fr ;
        rdakit:toolkitLabel       "famille vendeuse"@fr ;
        rdakit:toolkitDefinition  "Ancienne famille propriétaire d’un item qui a vendu cet item à un autre propriétaire."@fr ;
        reg:lexicalAlias          <http://rdaregistry.info/Elements/i/familleVendeuse.fr> .

<http://rdaregistry.info/Elements/i/P40109>
        rdfs:isDefinedBy          <http://rdaregistry.info/Elements/i/> ;
        reg:status                <http://metadataregistry.org/uri/RegStatus/1001> ;
        rdfs:label                "has seller person"@en ;
        reg:lexicalAlias          <http://rdaregistry.info/Elements/i/sellerPerson.en> ;
        skos:definition           "Relates an item to a person who is a former owner of an item who sells the item to another owner."@en ;
        rdakit:toolkitLabel       "seller person"@en ;
        rdakit:toolkitDefinition  "A person who is a former owner of an item who sells the item to another owner."@en ;
        rdf:type                  rdf:Property ;
        reg:name                  "sellerPerson" ;
        rdfs:domain               <http://rdaregistry.info/Elements/c/C10003> ;
        rdakit:hasElementType     "2" ;
        reg:hasSubproperty        <http://rdaregistry.info/Elements/i/datatype/P40109> ;
        reg:hasSubproperty        <http://rdaregistry.info/Elements/i/object/P40109> ;
        rdfs:subPropertyOf        <http://rdaregistry.info/Elements/i/P40102> ;
        rdfs:subPropertyOf        <http://rdaregistry.info/Elements/i/P40008> ;
        reg:hasUnconstrained      <http://rdaregistry.info/Elements/u/P60092> ;
        rdfs:label                "a pour personne vendeuse"@fr ;
        skos:definition           "Met un item en relation avec une ancienne personne propriétaire d’un item qui a vendu cet item à un autre propriétaire."@fr ;
        rdakit:toolkitLabel       "personne vendeuse"@fr ;
        rdakit:toolkitDefinition  "Ancienne personne propriétaire d’un item qui a vendu cet item à un autre propriétaire."@fr ;
        reg:lexicalAlias          <http://rdaregistry.info/Elements/i/personneVendeuse.fr> .

<http://rdaregistry.info/Elements/i/P40061>
        rdfs:isDefinedBy          <http://rdaregistry.info/Elements/i/> ;
        reg:status                <http://metadataregistry.org/uri/RegStatus/1001> ;
        rdf:type                  rdf:Property ;
        reg:name                  "subjectItemOf"@en ;
        rdfs:label                "is subject item of"@en ;
        reg:lexicalAlias          <http://rdaregistry.info/Elements/i/subjectItemOf.en> ;
        skos:definition           "Relates an item to a work that is about an item."@en ;
        rdfs:domain               <http://rdaregistry.info/Elements/c/C10003> ;
        reg:hasUnconstrained      <http://rdaregistry.info/Elements/u/P60806> ;
        rdakit:toolkitLabel       "subject item of"@en ;
        rdakit:toolkitDefinition  "A work that is about an item."@en ;
        rdfs:subPropertyOf        <http://rdaregistry.info/Elements/i/P40069> ;
        reg:hasSubproperty        <http://rdaregistry.info/Elements/i/P40062> ;
        reg:hasSubproperty        <http://rdaregistry.info/Elements/i/object/P40061> ;
        reg:name                  "chủĐềCủaBản"@vi ;
        rdfs:label                "là chủ đề của (bản)"@vi ;
        skos:definition           "Liên kết bản với tác phẩm về bản."@vi ;
        rdakit:toolkitLabel       "chủ đề của (bản)"@vi ;
        rdakit:toolkitDefinition  "Tác phẩm về bản."@vi ;
        reg:name                  "emneOmEksemplar"@da ;
        rdfs:label                "er emne om (eksempar)"@da ;
        reg:lexicalAlias          <http://rdaregistry.info/Elements/i/emneOmEksemplar.da> ;
        skos:definition           "Relaterer et eksemplar til et værk, der handler om et eksemplar."@da ;
        rdakit:toolkitLabel       "emne om (eksemplar)"@da ;
        rdakit:toolkitDefinition  "Værk, der er emne om et eksemplar."@da ;
        rdfs:label                "ist Thema von (Exemplar)"@de ;
        skos:definition           "Setzt ein Exemplar mit einem Werk, das von einem Exemplar handelt, in Beziehung."@de ;
        rdakit:toolkitLabel       "Thema von (Exemplar)"@de ;
        rdakit:toolkitDefinition  "Ein Werk, das von einem Exemplar handelt."@de ;
        reg:name                  "θέμαΤουΑντιτύπου"@el ;
        rdfs:label                "είναι θέμα του (αντίτυπο)"@el ;
        reg:lexicalAlias          <http://rdaregistry.info/Elements/i/θέμαΤουΑντιτύπου.el> ;
        skos:definition           "Συνδέει ένα αντίτυπο με ένα έργο σχετικά με ένα αντίτυπο."@el ;
        rdakit:toolkitLabel       "θέμα του (αντίτυπο)"@el ;
        rdakit:toolkitDefinition  "Ένα έργο σχετικά με ένα αντίτυπο."@el ;
        rdfs:label                "és matèria de (ítem)"@ca ;
        skos:definition           "Relaciona un item amb una obra que tracta d’un ítem."@ca ;
        rdakit:toolkitLabel       "matèria de (ítem)"@ca ;
        rdakit:toolkitDefinition  "Obra que tracta d’un ítem."@ca ;
        reg:name                  "kappaleAiheenaTeoksessa"@fi ;
        rdfs:label                "kappale aiheena teoksessa"@fi ;
        reg:lexicalAlias          <rdaa:kappaleAiheenaTeoksessa.fi> ;
        skos:definition           "Liittää kappaleen kappaleesta kertovaan teokseen."@fi ;
        rdakit:toolkitLabel       "kappale aiheena teoksessa"@fi ;
        rdakit:toolkitDefinition  "Kappaleesta kertova teos."@fi ;
        reg:name                  "sujetDeItem"@fr ;
        rdfs:label                "est un item sujet de"@fr ;
        reg:lexicalAlias          <http://rdaregistry.info/Elements/i/itemSujetDe.fr> ;
        skos:definition           "Met un item en relation avec une œuvre qui traite d’un item."@fr ;
        rdakit:toolkitDefinition  "Œuvre qui traite d’un item."@fr ;
        rdakit:toolkitLabel       "item sujet de"@fr ;
        rdakit:toolkitLabel       "emne for (eksemplar)"@no ;
        rdakit:toolkitDefinition  "Et verk som handler om et eksemplar."@no ;
        rdfs:subPropertyOf        <http://rdaregistry.info/Elements/x/P00014> ;
        rdakit:hasElementType     "2" ;
        skos:altLabel             "subject of (item)"@en ;
        reg:name                  "Példánytárgya"@hu ;
        rdfs:label                "tárgya (példány)"@hu ;
        skos:definition           "Egy példányt hozzákapcsol egy olyan példányhoz, amely egy példányról szól. "@hu ;
        rdakit:toolkitLabel       "tárgy (példány)"@hu ;
        rdakit:toolkitDefinition  "Egy mű, amely egy példányról szól."@hu ;
        skos:altLabel             "sujet de (item)"@fr .

<http://rdaregistry.info/Elements/i/P40082>
        rdfs:isDefinedBy          <http://rdaregistry.info/Elements/i/> ;
        reg:status                <http://metadataregistry.org/uri/RegStatus/1001> ;
        rdf:type                  rdf:Property ;
        reg:name                  "titleOfItem"@en ;
        rdfs:label                "has title of item"@en ;
        reg:lexicalAlias          <http://rdaregistry.info/Elements/i/titleOfItem.en> ;
        skos:definition           "Relates an item to an appellation of item in natural language and phrasing used in common discourse."@en ;
        rdfs:domain               <http://rdaregistry.info/Elements/c/C10003> ;
        rdakit:toolkitLabel       "title of item"@en ;
        rdakit:toolkitDefinition  "An appellation of item in natural language and phrasing used in common discourse."@en ;
        rdfs:subPropertyOf        <http://rdaregistry.info/Elements/i/P40081> ;
        reg:hasUnconstrained      <http://rdaregistry.info/Elements/u/P60367> ;
        reg:hasSubproperty        <http://rdaregistry.info/Elements/i/object/P40082> ;
        rdakit:hasElementType     "3" ;
        reg:hasSubproperty        <http://rdaregistry.info/Elements/i/datatype/P40082> ;
        reg:hasSubproperty        <http://rdaregistry.info/Elements/i/P40085> ;
        reg:hasSubproperty        <http://rdaregistry.info/Elements/i/P40086> ;
        rdfs:subPropertyOf        <http://rdaregistry.info/Elements/x/P00019> ;
        rdfs:label                "a pour titre d’item"@fr ;
        skos:definition           "Met un item en relation avec une appellation d’item exprimée dans un langage et une formulation naturels et utilisée dans le langage courant."@fr ;
        rdakit:toolkitLabel       "titre d’item"@fr ;
        rdakit:toolkitDefinition  "Appellation d’item exprimée dans un langage et une formulation naturels et utilisée dans le langage courant."@fr ;
        reg:lexicalAlias          <http://rdaregistry.info/Elements/i/titreDitem.fr> .

<http://rdaregistry.info/Elements/i/P40084>
        rdfs:isDefinedBy          <http://rdaregistry.info/Elements/i/> ;
        reg:status                <http://metadataregistry.org/uri/RegStatus/1001> ;
        rdf:type                  rdf:Property ;
        reg:name                  "variantAccessPointForItem"@en ;
        rdfs:label                "has variant access point for item"@en ;
        reg:lexicalAlias          <http://rdaregistry.info/Elements/i/variantAccessPointForItem.en> ;
        skos:definition           "Relates an item to an access point of item that is not selected for preference in a specific vocabulary encoding scheme."@en ;
        rdfs:domain               <http://rdaregistry.info/Elements/c/C10003> ;
        rdakit:toolkitLabel       "variant access point for item"@en ;
        rdakit:toolkitDefinition  "An access point of item that is not selected for preference in a specific vocabulary encoding scheme."@en ;
        rdfs:subPropertyOf        <http://rdaregistry.info/Elements/i/P40080> ;
        reg:hasUnconstrained      <http://rdaregistry.info/Elements/u/P60917> ;
        reg:hasSubproperty        <http://rdaregistry.info/Elements/i/object/P40084> ;
        rdakit:hasElementType     "3" ;
        reg:hasSubproperty        <http://rdaregistry.info/Elements/i/datatype/P40084> ;
        rdfs:subPropertyOf        <http://rdaregistry.info/Elements/x/P00022> ;
        rdfs:label                "a pour variante de point d’accès d’un item"@fr ;
        skos:definition           "Met un item en relation avec un point d’accès d’un item qui ne fait pas l’objet d’un choix privilégié dans un schéma d’encodage de vocabulaire spécifique."@fr ;
        rdakit:toolkitLabel       "variante de point d’accès d’un item"@fr ;
        rdakit:toolkitDefinition  "Point d’accès d’un item qui ne fait pas l’objet d’un choix privilégié dans un schéma d’encodage de vocabulaire spécifique."@fr ;
        reg:lexicalAlias          <http://rdaregistry.info/Elements/i/varianteDePointDaccèsDunItem.fr> .

<http://rdaregistry.info/Elements/i/P40086>
        rdfs:isDefinedBy          <http://rdaregistry.info/Elements/i/> ;
        reg:status                <http://metadataregistry.org/uri/RegStatus/1001> ;
        rdf:type                  rdf:Property ;
        reg:name                  "variantTitleOfItem"@en ;
        rdfs:label                "has variant title of item"@en ;
        reg:lexicalAlias          <http://rdaregistry.info/Elements/i/variantTitleOfItem.en> ;
        skos:definition           "Relates an item to a title of item that is not selected for preference in a specific application or context."@en ;
        rdfs:domain               <http://rdaregistry.info/Elements/c/C10003> ;
        rdakit:toolkitLabel       "variant title of item"@en ;
        rdakit:toolkitDefinition  "A title of item that is not selected for preference in a specific application or context."@en ;
        rdfs:subPropertyOf        <http://rdaregistry.info/Elements/i/P40082> ;
        reg:hasUnconstrained      <http://rdaregistry.info/Elements/u/P60355> ;
        reg:hasSubproperty        <http://rdaregistry.info/Elements/i/object/P40086> ;
        rdakit:hasElementType     "3" ;
        reg:hasSubproperty        <http://rdaregistry.info/Elements/i/datatype/P40086> ;
        rdfs:subPropertyOf        <http://rdaregistry.info/Elements/x/P00023> ;
        rdfs:label                "a pour variante de titre d’item"@fr ;
        skos:definition           "Met un item en relation avec un titre d’item qui ne fait pas l’objet d’un choix privilégié dans une application ou un contexte spécifiques."@fr ;
        rdakit:toolkitLabel       "variante de titre d’item"@fr ;
        rdakit:toolkitDefinition  "Titre d’item qui ne fait pas l’objet d’un choix privilégié dans une application ou un contexte spécifiques."@fr ;
        reg:lexicalAlias          <http://rdaregistry.info/Elements/i/varianteDeTitreDitem.fr> .

<http://rdaregistry.info/Elements/i/P40054>
        rdfs:isDefinedBy          <http://rdaregistry.info/Elements/i/> ;
        reg:status                <http://metadataregistry.org/uri/RegStatus/1008> ;
        reg:name                  "wholePartItemRelationship"@en ;
        rdf:type                  rdf:Property ;
        rdfs:domain               <http://rdaregistry.info/Elements/c/C10003> ;
        reg:hasSubproperty        <http://rdaregistry.info/Elements/i/P40009> ;
        reg:hasSubproperty        <http://rdaregistry.info/Elements/i/P40034> ;
        reg:lexicalAlias          <http://rdaregistry.info/Elements/i/wholePartItemRelationship.en> ;
        reg:hasUnconstrained      <http://rdaregistry.info/Elements/u/P60714> ;
        rdfs:label                "a pour relation d’item tout-partie"@fr ;
        skos:definition           "Met un item en relation avec un item qui contient ou est contenu dans un autre item."@fr ;
        rdakit:toolkitLabel       "relation d’item tout-partie"@fr ;
        rdakit:toolkitDefinition  "Item qui contient ou est contenu dans un autre item."@fr ;
        rdakit:toolkitLabel       "relación del ítem todo-parte"@es ;
        rdakit:toolkitDefinition  "Un ítem que es incluido en, o contiene el ítem."@es ;
        rdfs:subPropertyOf        <http://rdaregistry.info/Elements/i/P40046> ;
        rdakit:instructionNumber  "24.5" ;
        reg:hasSubproperty        <http://rdaregistry.info/Elements/i/object/P40054> ;
        reg:name                  "mốiQuanHệBảnToànBộPhần"@vi ;
        rdfs:label                "có mối quan hệ bản toàn bộ-phần với"@vi ;
        skos:definition           "Liên kết bản với bản được chứa trong hoặc có chứa bản khác."@vi ;
        rdakit:toolkitLabel       "mối quan hệ bản toàn bộ phần"@vi ;
        rdakit:toolkitDefinition  "Bản được chứa trong hoặc có chứa bản khác."@vi ;
        reg:name                  "helhedDelEksemplarrelation"@da ;
        rdfs:label                "har helhed-del-eksemplarrelation med"@da ;
        reg:lexicalAlias          <http://rdaregistry.info/Elements/i/helhedDelEksemplarrelation.da> ;
        skos:definition           "Relaterer et eksemplar til et eksemplar der indgår i, eller indeholder et eksemplar."@da ;
        rdakit:toolkitLabel       "helhed-del-eksemplarrelation"@da ;
        rdakit:toolkitDefinition  "Eksemplar der indgår i, eller indeholder et eksemplar."@da ;
        rdfs:label                "hat Teil-Ganzes-Beziehung auf Exemplarebene"@de ;
        skos:definition           "Setzt ein Exemplar mit einem Exemplar, das in einem anderen Exemplar enthalten ist oder eins enthält, in Beziehung."@de ;
        rdakit:toolkitLabel       "Teil-Ganzes-Beziehung auf Exemplarebene"@de ;
        rdakit:toolkitDefinition  "Ein Exemplar, das in einem anderen Exemplar enthalten ist oder eins enthält."@de ;
        reg:name                  "σχέσηΣυνόλουΤμήματοςΑντιτύπου"@el ;
        rdfs:label                "έχει σχέση συνόλου-τμήματος του αντιτύπου με"@el ;
        reg:lexicalAlias          <http://rdaregistry.info/Elements/i/σχέσηΣυνόλουΤμήματοςΑντιτύπου.el> ;
        skos:definition           "Συνδέει ένα αντίτυπο με ένα αντίτυπο το οποίο περιέχεται σε ή περιέχει κάποιο άλλο αντίτυπο."@el ;
        rdakit:toolkitLabel       "σχέση συνόλου-τμήματος του αντιτύπου"@el ;
        rdakit:toolkitDefinition  "Ένα αντίτυπο το οποίο περιέχεται σε ή περιέχει κάποιο άλλο αντίτυπο."@el ;
        rdfs:label                "té com a relació d’ítem tot-part"@ca ;
        skos:definition           "Relaciona un item amb un ítem que és contingut o conté un altre ítem."@ca ;
        rdakit:toolkitLabel       "relació d’ítem tot-part"@ca ;
        rdakit:toolkitDefinition  "Ítem que és contingut o conté un altre ítem."@ca ;
        reg:name                  "osaKokonaissuhdeKappaleeseen"@fi ;
        rdfs:label                "osa-kokonaissuhde kappaleeseen"@fi ;
        reg:lexicalAlias          <rdaa:osaKokonaissuhdeKappaleeseen.fi> ;
        skos:definition           "Liittää kappaleen kappaleeseen, joka sisältyy toiseen kappaleeseen tai sisältää toisen kappaleen."@fi ;
        rdakit:toolkitLabel       "osa-kokonaissuhde kappaleeseen"@fi ;
        rdakit:toolkitDefinition  "Kappale, joka sisältyy toiseen kappaleeseen tai sisältää toisen kappaleen."@fi ;
        reg:name                  "relationDitemToutpartie"@fr ;
        reg:lexicalAlias          <http://rdaregistry.info/Elements/i/relationDitemToutpartie.fr> ;
        rdakit:toolkitLabel       "relasjonstypen hel/del av eksemplar"@no ;
        rdakit:toolkitDefinition  "Et eksemplar som omfattes av eller selv omfatter et annet eksemplar."@no ;
        reg:hasSubproperty        <http://rdaregistry.info/Elements/i/datatype/P40054> .

<http://metadataregistry.org/uri/RegStatus/1001>
        rdf:type        skos:Concept ;
        skos:prefLabel  "Published"@en .

<http://metadataregistry.org/uri/RegStatus/1008>
        rdf:type        skos:Concept ;
        skos:prefLabel  "Deprecated"@en .
