@prefix dc: <http://purl.org/dc/elements/1.1/> .
@prefix foaf: <http://xmlns.com/foaf/0.1/> .
@prefix rdakit: <http://metadataregistry.org/uri/profile/rdakit/> .
@prefix rdf: <http://www.w3.org/1999/02/22-rdf-syntax-ns#> .
@prefix rdfs: <http://www.w3.org/2000/01/rdf-schema#> .
@prefix reg: <http://metadataregistry.org/uri/profile/regap/> .
@prefix skos: <http://www.w3.org/2004/02/skos/core#> .
@prefix xml: <http://www.w3.org/XML/1998/namespace> .
@prefix xsd: <http://www.w3.org/2001/XMLSchema#> .

<http://rdaregistry.info/Elements/e/P20001> a rdf:Property ;
    rdfs:label "has content type"@en,
        "har innehållstyp"@sv ;
    rdakit:instructionNumber "6.9" ;
    rdakit:toolkitDefinition "A categorization reflecting the fundamental form of communication in which the content is expressed and the human sense through which it is intended to be perceived."@en,
        "Una categorización que refleja la forma fundamental de comunicación en la cual se expresa el contenido y el sentido humano a través por el se espera sea percibido."@es,
        "Catégorisation reflétant la forme fondamentale de communication sous laquelle le contenu est exprimé et le sens humain par lequel il doit être perçu."@fr ;
    rdakit:toolkitLabel "content type"@en,
        "tipo de contenido"@es,
        "type de contenu"@fr,
        "innehållstyp"@sv ;
    reg:hasUnconstrained <http://rdaregistry.info/Elements/u/P60049> ;
    reg:lexicalAlias <http://rdaregistry.info/Elements/e/contentType.en> ;
    reg:name "contentType"@en ;
    reg:status <http://metadataregistry.org/uri/RegStatus/1001> ;
    rdfs:domain <http://rdaregistry.info/Elements/c/C10006> ;
    rdfs:isDefinedBy <http://rdaregistry.info/Elements/e/> ;
    skos:definition "Relates an expression to a categorization reflecting the fundamental form of communication in which the content is expressed and the human sense through which it is intended to be perceived."@en ;
    skos:scopeNote "Content type also reflects the number of spatial dimensions and the presence or absence of movement in which content expressed in the form of an image or images is intended to be perceived."@en .

<http://rdaregistry.info/Elements/e/P20002> a rdf:Property ;
    rdfs:label "has identifier for expression"@en,
        "har identifikator för uttrycket"@sv ;
    rdakit:instructionNumber "6.13" ;
    rdakit:toolkitDefinition "A character string uniquely associated with an expression, or with a surrogate such as an authority record for an expression."@en,
        "Una cadena de caracteres unívocamente asociada con una expresión, o con un substituto de una expresión (p.ej., un registro de autoridad)."@es,
        "Chaîne de caractères associée de manière unique à une expression ou à un substitut d’une expression (par exemple, une notice d’autorité), qui sert à distinguer cette expression d’autres expressions."@fr ;
    rdakit:toolkitLabel "identifier for expression"@en,
        "identificador de la expresión"@es,
        "identifiant de l’expression"@fr,
        "identifikator för uttrycket"@sv ;
    reg:hasUnconstrained <http://rdaregistry.info/Elements/u/P60052> ;
    reg:lexicalAlias <http://rdaregistry.info/Elements/e/identifierForExpression.en> ;
    reg:name "identifierForExpression"@en ;
    reg:status <http://metadataregistry.org/uri/RegStatus/1001> ;
    rdfs:domain <http://rdaregistry.info/Elements/c/C10006> ;
    rdfs:isDefinedBy <http://rdaregistry.info/Elements/e/> ;
    skos:definition "Relates an expression to a character string uniquely associated with an expression, or with a surrogate such as an authority record for an expression."@en ;
    skos:scopeNote "An identifier serves to differentiate an expression from other expressions."@en .

<http://rdaregistry.info/Elements/e/P20003> a rdf:Property ;
    rdfs:label "has other distinguishing characteristic of expression"@en,
        "har andra särskiljande egenskaper för uttrycket"@sv ;
    rdakit:instructionNumber "6.12" ;
    rdakit:toolkitDefinition "A characteristic other than content type, language of expression, or date of expression serving to differentiate an expression from another expression of the same work."@en,
        "Una característica diferente del tipo de contenido, lengua de expresión o fecha de expresión."@es,
        "Caractéristique autre que le type de contenu, la langue de l’expression ou la date de l’expression."@fr ;
    rdakit:toolkitLabel "other distinguishing characteristic of expression"@en,
        "otra característica distintiva de la expresión"@es,
        "autre caractéristique distinctive de l’expression"@fr,
        "andra särskiljande egenskaper för uttrycket"@sv ;
    reg:hasUnconstrained <http://rdaregistry.info/Elements/u/P60054> ;
    reg:lexicalAlias <http://rdaregistry.info/Elements/e/otherDistinguishingCharacteristicOfExpression.en> ;
    reg:name "otherDistinguishingCharacteristicOfExpression"@en ;
    reg:status <http://metadataregistry.org/uri/RegStatus/1001> ;
    rdfs:domain <http://rdaregistry.info/Elements/c/C10006> ;
    rdfs:isDefinedBy <http://rdaregistry.info/Elements/e/> ;
    skos:definition "Relates an expression to a characteristic other than content type, language of expression, or date of expression serving to differentiate an expression from another expression of the same work."@en ;
    skos:scopeNote "Elle sert à distinguer une expression d’une autre expression de la même œuvre."@fr .

<http://rdaregistry.info/Elements/e/P20004> a rdf:Property ;
    rdfs:label "has date of capture"@en,
        "har inspelningstid"@sv ;
    rdakit:instructionNumber "7.11.3" ;
    rdakit:toolkitDefinition "A date associated with the recording, filming, etc., of the content of an expression."@en,
        "Una fecha o rango de fechas asociadas con la captura (i.e, grabación, filmación, etc.) del contenido del recurso."@es,
        "La date ou la fourchette de dates associée à la captation (c’est-à-dire l’enregistrement, le tournage, etc.) du contenu de la ressource."@fr ;
    rdakit:toolkitLabel "date of capture"@en,
        "fecha de captura"@es,
        "date de captation"@fr,
        "inspelningstid"@sv ;
    reg:hasUnconstrained <http://rdaregistry.info/Elements/u/P60074> ;
    reg:lexicalAlias <http://rdaregistry.info/Elements/e/dateOfCapture.en> ;
    reg:name "dateOfCapture"@en ;
    reg:status <http://metadataregistry.org/uri/RegStatus/1001> ;
    rdfs:domain <http://rdaregistry.info/Elements/c/C10006> ;
    rdfs:isDefinedBy <http://rdaregistry.info/Elements/e/> ;
    skos:definition "Relates an expression to a date associated with the recording, filming, etc., of the content of an expression."@en .

<http://rdaregistry.info/Elements/e/P20005> a rdf:Property ;
    rdfs:label "has award"@en,
        "har utmärkelse"@sv ;
    rdakit:instructionNumber "7.28" ;
    rdakit:toolkitDefinition "A formal recognition of excellence, etc., given by an award- or prize-granting body, for the content of an expression."@en,
        "Un reconocimiento formal de excelencia, etc., otorgado por una entidad que concede premios o reconocimientos, por el contenido de un recurso."@es,
        "Reconnaissance officielle d’excellence, etc. accordée au contenu d’une ressource par un organisme octroyant une récompense ou un prix."@fr ;
    rdakit:toolkitLabel "award"@en,
        "premio"@es,
        "prix"@fr,
        "utmärkelse"@sv ;
    reg:hasUnconstrained <http://rdaregistry.info/Elements/u/P60090> ;
    reg:lexicalAlias <http://rdaregistry.info/Elements/e/award.en> ;
    reg:name "award"@en ;
    reg:status <http://metadataregistry.org/uri/RegStatus/1001> ;
    rdfs:domain <http://rdaregistry.info/Elements/c/C10006> ;
    rdfs:isDefinedBy <http://rdaregistry.info/Elements/e/> ;
    skos:definition "Relates an expression to a formal recognition of excellence, etc., given by an award- or prize-granting body, for the content of an expression."@en .

<http://rdaregistry.info/Elements/e/P20006> a rdf:Property ;
    rdfs:label "has language of expression"@en ;
    rdakit:instructionNumber "6.11" ;
    rdakit:toolkitDefinition "A language in which a work is expressed."@en,
        "Una lengua en la que se expresa una obra"@es,
        "Langue dans laquelle une œuvre est exprimée."@fr ;
    rdakit:toolkitLabel "language of expression"@en,
        "lengua de la expresión"@es,
        "langue de l’expression"@fr ;
    reg:hasUnconstrained <http://rdaregistry.info/Elements/u/P60099> ;
    reg:lexicalAlias <http://rdaregistry.info/Elements/e/languageOfExpression.en> ;
    reg:name "languageOfExpression"@en ;
    reg:status <http://metadataregistry.org/uri/RegStatus/1001> ;
    rdfs:domain <http://rdaregistry.info/Elements/c/C10006> ;
    rdfs:isDefinedBy <http://rdaregistry.info/Elements/e/> ;
    skos:definition "Relates an expression to a language in which a work is expressed."@en .

<http://rdaregistry.info/Elements/e/P20008> a rdf:Property ;
    reg:status <http://metadataregistry.org/uri/RegStatus/1008> ;
    rdfs:isDefinedBy <http://rdaregistry.info/Elements/e/> .

<http://rdaregistry.info/Elements/e/P20057> a rdf:Property ;
    reg:status <http://metadataregistry.org/uri/RegStatus/1008> ;
    rdfs:isDefinedBy <http://rdaregistry.info/Elements/e/> .

<http://rdaregistry.info/Elements/e/P20059> a rdf:Property ;
    rdfs:label "has manifestation of expression"@en,
        "har manifestation av uttryck"@sv ;
    rdakit:instructionNumber "17.9" ;
    rdakit:toolkitDefinition "A physical embodiment of an expression."@en,
        "Una materialización física de una expresión."@es,
        "Matérialisation d’une expression."@fr ;
    rdakit:toolkitLabel "manifestation of expression"@en,
        "manifestación de la expresión"@es,
        "manifestation d’une expression"@fr,
        "manifestation av uttryck"@sv ;
    reg:hasSubproperty <http://rdaregistry.info/Elements/e/object/P20059> ;
    reg:lexicalAlias <http://rdaregistry.info/Elements/e/manifestationOfExpression.en> ;
    reg:name "manifestationOfExpression"@en ;
    reg:status <http://metadataregistry.org/uri/RegStatus/1001> ;
    rdfs:domain <http://rdaregistry.info/Elements/c/C10006> ;
    rdfs:isDefinedBy <http://rdaregistry.info/Elements/e/> ;
    skos:definition "Relates an expression to a physical embodiment of an expression."@en .

<http://rdaregistry.info/Elements/e/P20069> a rdf:Property ;
    rdfs:label "has summarization of content"@en,
        "har innehållsbeskrivning"@sv ;
    rdakit:instructionNumber "7.10" ;
    rdakit:toolkitDefinition "An abstract, summary, synopsis, etc., of the content of an expression."@en,
        "Un resumen, sumario, sinopsis, etc., del contenido de un recurso."@es,
        "Synthèse, résumé, synopsis, etc. du contenu d’une ressource."@fr ;
    rdakit:toolkitLabel "summarization of content"@en,
        "resumen del contenido"@es,
        "résumé du contenu"@fr,
        "innehållsbeskrivning"@sv ;
    reg:hasUnconstrained <http://rdaregistry.info/Elements/u/P60372> ;
    reg:lexicalAlias <http://rdaregistry.info/Elements/e/summarizationOfContent.en> ;
    reg:name "summarizationOfContent"@en ;
    reg:status <http://metadataregistry.org/uri/RegStatus/1001> ;
    rdfs:domain <http://rdaregistry.info/Elements/c/C10006> ;
    rdfs:isDefinedBy <http://rdaregistry.info/Elements/e/> ;
    skos:definition "Relates an expression to an abstract, summary, synopsis, etc., of the content of an expression."@en .

<http://rdaregistry.info/Elements/e/P20206> a rdf:Property ;
    rdfs:label "has supplementary content"@en,
        "har bihang"@sv ;
    rdakit:instructionNumber "7.16" ;
    rdakit:toolkitDefinition "An indication of content that updates or complements the primary content of an expression."@en,
        "Contenido (por j., un índice, una bibliografía, un apéndice) destinado a suplementar el contenido primario de un recurso."@es,
        "Contenu (par exemple, un index, une bibliographie, une annexe) conçu pour compléter le contenu principal d’une ressource."@fr ;
    rdakit:toolkitLabel "supplementary content"@en,
        "contenido suplementario"@es,
        "contenu supplémentaire"@fr,
        "bihang"@sv ;
    reg:hasUnconstrained <http://rdaregistry.info/Elements/u/P60485> ;
    reg:lexicalAlias <http://rdaregistry.info/Elements/e/supplementaryContent.en> ;
    reg:name "supplementaryContent"@en ;
    reg:status <http://metadataregistry.org/uri/RegStatus/1001> ;
    rdfs:domain <http://rdaregistry.info/Elements/c/C10006> ;
    rdfs:isDefinedBy <http://rdaregistry.info/Elements/e/> ;
    skos:definition "Relates an expression to an indication of content that updates or complements the primary content of an expression."@en ;
    skos:scopeNote "Supplementary content may include an index, a bibliography, or an appendix."@en .

<http://rdaregistry.info/Elements/e/P20207> a rdf:Property ;
    rdfs:label "has illustrative content"@en,
        "har illustrativt innehåll"@sv ;
    rdakit:instructionNumber "7.15" ;
    rdakit:toolkitDefinition "A presence of image content that accompanies the primary content of an expression."@en,
        "Contenido destinado a ilustrar el contenido primario de un recurso.."@es,
        "Contenu destiné à illustrer le contenu principal d’une ressource."@fr ;
    rdakit:toolkitLabel "illustrative content"@en,
        "contenido ilustrativo"@es,
        "contenu illustratif"@fr,
        "illustrativt innehåll"@sv ;
    reg:hasUnconstrained <http://rdaregistry.info/Elements/u/P60486> ;
    reg:lexicalAlias <http://rdaregistry.info/Elements/e/illustrativeContent.en> ;
    reg:name "illustrativeContent"@en ;
    reg:status <http://metadataregistry.org/uri/RegStatus/1001> ;
    rdfs:domain <http://rdaregistry.info/Elements/c/C10006> ;
    rdfs:isDefinedBy <http://rdaregistry.info/Elements/e/> ;
    skos:definition "Relates an expression to a presence of one or more still images that accompany the primary content of an expression."@en ;
    skos:scopeNote "Tables containing only words and/or numerical data are excluded."@en .

<http://rdaregistry.info/Elements/e/P20208> a rdf:Property ;
    rdfs:label "has accessibility content"@en,
        "har komplement för tillgänglighet"@sv ;
    rdakit:instructionNumber "7.14" ;
    rdakit:seeAlso <http://rdaregistry.info/Elements/e/P20007> ;
    rdakit:toolkitDefinition "An indication of content that provides alternative sensory modes to perceive the primary content of an expression."@en,
        "Contenido que ayuda a las personas con discapacidad sensorial para lograr una mayor comprensión de un contenido que su discapacidad les impide oir y ver en forma completa."@es,
        "Contenu permettant aux handicapés sensoriels une meilleure compréhension d’un contenu que leur handicap les empêche de voir ou d’entendre parfaitement."@fr ;
    rdakit:toolkitLabel "accessibility content"@en,
        "contenido con accesibilidad ampliada"@es,
        "contenu accessible"@fr,
        "komplement för tillgänglighet"@sv ;
    reg:hasUnconstrained <http://rdaregistry.info/Elements/u/P60487> ;
    reg:lexicalAlias <http://rdaregistry.info/Elements/e/accessibilityContent.en> ;
    reg:name "accessibilityContent"@en ;
    reg:status <http://metadataregistry.org/uri/RegStatus/1001> ;
    rdfs:domain <http://rdaregistry.info/Elements/c/C10006> ;
    rdfs:isDefinedBy <http://rdaregistry.info/Elements/e/> ;
    skos:definition "Relates an expression to an indication of content that provides alternative sensory modes to perceive the primary content of an expression."@en ;
    skos:scopeNote "Accessibility content includes accessible labels, audio description, captioning, image description, sign language, and subtitles. Accessibility content does not include subtitles in a language different from the spoken content."@en .

<http://rdaregistry.info/Elements/e/P20209> a rdf:Property ;
    rdfs:label "has format of notated music"@en,
        "har format för noterad musik"@sv ;
    rdakit:instructionNumber "7.20" ;
    rdakit:toolkitDefinition "A musical or physical layout of the content of an expression that is presented in the form of musical notation."@en,
        "La presentación musical o física del contenido de un recurso que se presenta en forma de notación musical."@es,
        "La disposition musicale ou matérielle du contenu d’une ressource qui se présente sous la forme d’une notation musicale."@fr ;
    rdakit:toolkitLabel "format of notated music"@en,
        "formato de música notada"@es,
        "présentation de la musique notée"@fr,
        "format för noterad musik"@sv ;
    reg:hasUnconstrained <http://rdaregistry.info/Elements/u/P60488> ;
    reg:lexicalAlias <http://rdaregistry.info/Elements/e/formatOfNotatedMusic.en> ;
    reg:name "formatOfNotatedMusic"@en ;
    reg:status <http://metadataregistry.org/uri/RegStatus/1001> ;
    rdfs:domain <http://rdaregistry.info/Elements/c/C10006> ;
    rdfs:isDefinedBy <http://rdaregistry.info/Elements/e/> ;
    skos:definition "Relates an expression to a musical or physical layout of the content of an expression that is presented in the form of musical notation."@en .

<http://rdaregistry.info/Elements/e/P20210> a rdf:Property ;
    rdfs:label "has other details of cartographic content"@en,
        "har övrig kartografisk data"@sv ;
    rdakit:instructionNumber "7.27" ;
    rdakit:toolkitDefinition "An indication of mathematical data and other features of the cartographic content of an expression not recorded in statements of scale, projection, and coordinates."@en,
        "Datos matemáticos y otras características del contenido cartográfico de un recurso, que no se han registrado en las menciones de escala, proyección y coordenadas."@es,
        "Données mathématiques et autres particularités du contenu cartographique d’une ressource qui ne sont pas enregistrées dans les mentions d’échelle, de projection et de coordonnées."@fr ;
    rdakit:toolkitLabel "other details of cartographic content"@en,
        "otros detalles del contenido cartográfico"@es,
        "autres particularités du contenu cartographique"@fr,
        "övrig kartografisk data"@sv ;
    reg:hasUnconstrained <http://rdaregistry.info/Elements/u/P60498> ;
    reg:lexicalAlias <http://rdaregistry.info/Elements/e/otherDetailsOfCartographicContent.en> ;
    reg:name "otherDetailsOfCartographicContent"@en ;
    reg:status <http://metadataregistry.org/uri/RegStatus/1001> ;
    rdfs:domain <http://rdaregistry.info/Elements/c/C10006> ;
    rdfs:isDefinedBy <http://rdaregistry.info/Elements/e/> ;
    skos:definition "Relates an expression to an indication of mathematical data and other features of the cartographic content of an expression not recorded in statements of scale, projection, and coordinates."@en .

<http://rdaregistry.info/Elements/e/P20214> a rdf:Property ;
    rdfs:label "has date of expression"@en ;
    rdakit:instructionNumber "6.10" ;
    rdakit:toolkitDefinition "An earliest date associated with an expression."@en,
        "La fecha más antigua asociada con una expresión."@es,
        "La date la plus ancienne associée à une expression."@fr ;
    rdakit:toolkitLabel "date of expression"@en,
        "fecha de la expresión"@es,
        "date de l’expression"@fr ;
    reg:hasUnconstrained <http://rdaregistry.info/Elements/u/P60527> ;
    reg:lexicalAlias <http://rdaregistry.info/Elements/e/dateOfExpression.en> ;
    reg:name "dateOfExpression"@en ;
    reg:status <http://metadataregistry.org/uri/RegStatus/1001> ;
    rdfs:domain <http://rdaregistry.info/Elements/c/C10006> ;
    rdfs:isDefinedBy <http://rdaregistry.info/Elements/e/> ;
    skos:definition "Relates an expression to an earliest date associated with an expression."@en .

<http://rdaregistry.info/Elements/e/P20215> a rdf:Property ;
    rdfs:label "has medium of performance of musical content"@en ;
    rdakit:instructionNumber "7.21" ;
    rdakit:toolkitDefinition "An instrument, voice, and/or ensemble used, or intended to be used, for performance of musical content."@en,
        "El instrumento, instrumentos, voz, voces, etc., utilizados para (o con el propósito de ser utilizados para) la ejecución del contenido musical."@es,
        "Le ou les instruments, la ou les voix, etc. utilisés (ou destinés à être utilisés) dans une exécution d’un contenu musical."@fr ;
    rdakit:toolkitLabel "medium of performance of musical content"@en,
        "medio de interpretación del contenido musical"@es,
        "distribution d’exécution d’un contenu musical"@fr ;
    reg:hasUnconstrained <http://rdaregistry.info/Elements/u/P60537> ;
    reg:lexicalAlias <http://rdaregistry.info/Elements/e/mediumOfPerformanceOfMusicalContent.en> ;
    reg:name "mediumOfPerformanceOfMusicalContent"@en ;
    reg:status <http://metadataregistry.org/uri/RegStatus/1001> ;
    rdfs:domain <http://rdaregistry.info/Elements/c/C10006> ;
    rdfs:isDefinedBy <http://rdaregistry.info/Elements/e/> ;
    skos:definition "Relates an expression to an instrument, voice, or ensemble used, or intended to be used, for performance of musical content."@en .

<http://rdaregistry.info/Elements/e/P20216> a rdf:Property ;
    rdfs:label "has projection of cartographic content"@en,
        "har kartprojektion"@sv ;
    rdakit:instructionNumber "7.26" ;
    rdakit:toolkitDefinition "A method or system used to represent the surface of the Earth or of a celestial sphere on a plane."@en,
        "El medio o sistema utilizado para representar la superficie de la Tierra o de una esfera celeste en un plano."@es,
        "La méthode ou le système utilisé pour représenter la surface de la Terre ou d’une sphère céleste sur un plan."@fr ;
    rdakit:toolkitLabel "projection of cartographic content"@en,
        "proyección del contenido cartográfico"@es,
        "projection d’un contenu cartographique"@fr,
        "kartprojektion"@sv ;
    reg:hasUnconstrained <http://rdaregistry.info/Elements/u/P60542> ;
    reg:lexicalAlias <http://rdaregistry.info/Elements/e/projectionOfCartographicContent.en> ;
    reg:name "projectionOfCartographicContent"@en ;
    reg:status <http://metadataregistry.org/uri/RegStatus/1001> ;
    rdfs:domain <http://rdaregistry.info/Elements/c/C10006> ;
    rdfs:isDefinedBy <http://rdaregistry.info/Elements/e/> ;
    skos:definition "Relates an expression to a method or system used to represent the surface of the earth or of a celestial sphere on a plane."@en .

<http://rdaregistry.info/Elements/e/P20217> a rdf:Property ;
    rdfs:label "has capture information"@en,
        "har inspelningsort och inspelningstid"@sv ;
    rdakit:instructionNumber "7.11" ;
    rdakit:toolkitDefinition "A place, date, or other information associated with the recording, filming, etc., of the content of an expression."@en,
        "El lugar y fecha asociados con la captura (i.e., grabación, filmación, etc.) del contenido de un recurso."@es,
        "Le lieu et la date associés à la captation (c’est-à-dire l’enregistrement, le tournage, etc.) du contenu de la ressource."@fr ;
    rdakit:toolkitLabel "capture information"@en,
        "lugar y fecha de captura"@es,
        "lieu et date de la captation"@fr,
        "inspelningsort och inspelningstid"@sv ;
    reg:hasUnconstrained <http://rdaregistry.info/Elements/u/P60555> ;
    reg:lexicalAlias <http://rdaregistry.info/Elements/e/captureInformation.en> ;
    reg:name "capture information"@en ;
    reg:status <http://metadataregistry.org/uri/RegStatus/1001> ;
    rdfs:domain <http://rdaregistry.info/Elements/c/C10006> ;
    rdfs:isDefinedBy <http://rdaregistry.info/Elements/e/> ;
    skos:definition "Relates an expression to a place, date, or other information associated with the recording, filming, etc., of the content of an expression. "@en .

<http://rdaregistry.info/Elements/e/P20218> a rdf:Property ;
    rdfs:label "has place of capture"@en,
        "har inspelningsort"@sv ;
    rdakit:instructionNumber "7.11.2" ;
    rdakit:toolkitDefinition "A place associated with the recording, filming, etc., of the content of an expression."@en,
        "El lugar asociado con la captura (i.e, grabación, filmación, etc.) del contenido del recurso."@es,
        "Le lieu associé à la captation (c’est-à-dire l’enregistrement, le tournage, etc.) du contenu d’une ressource."@fr ;
    rdakit:toolkitLabel "place of capture"@en,
        "lugar de captura"@es,
        "lieu de captation"@fr,
        "inspelningsort"@sv ;
    reg:hasUnconstrained <http://rdaregistry.info/Elements/u/P60556> ;
    reg:lexicalAlias <http://rdaregistry.info/Elements/e/placeOfCapture.en> ;
    reg:name "placeOfCapture"@en ;
    reg:status <http://metadataregistry.org/uri/RegStatus/1001> ;
    rdfs:domain <http://rdaregistry.info/Elements/c/C10006> ;
    rdfs:isDefinedBy <http://rdaregistry.info/Elements/e/> ;
    skos:definition "Relates an expression to a place associated with the recording, filming, etc., of the content of an expression."@en .

<http://rdaregistry.info/Elements/e/P20219> a rdf:Property ;
    rdfs:label "has duration"@en,
        "har speltid"@sv ;
    rdakit:instructionNumber "7.22" ;
    rdakit:toolkitDefinition "A playing time, performance time, running time, etc., of the content of an expression."@en,
        "El tiempo de reproducción, el tiempo de interpretación, etc., del contenido de un recurso."@es,
        "La durée de lecture, de projection, etc. du contenu de la ressource."@fr ;
    rdakit:toolkitLabel "duration"@en,
        "duración"@es,
        "durée"@fr,
        "speltid"@sv ;
    reg:hasUnconstrained <http://rdaregistry.info/Elements/u/P60557> ;
    reg:lexicalAlias <http://rdaregistry.info/Elements/e/duration.en> ;
    reg:name "duration"@en ;
    reg:status <http://metadataregistry.org/uri/RegStatus/1001> ;
    rdfs:domain <http://rdaregistry.info/Elements/c/C10006> ;
    rdfs:isDefinedBy <http://rdaregistry.info/Elements/e/> ;
    skos:definition "Relates an expression to a playing time, performance time, running time, etc., of the content of an expression."@en .

<http://rdaregistry.info/Elements/e/P20225> a rdf:Property ;
    rdfs:label "has sound content"@en,
        "har ljudinnehåll"@sv ;
    rdakit:instructionNumber "7.18" ;
    rdakit:toolkitDefinition "A presence or absence of sound in an expression."@en,
        "La presencia de sonido en un recurso, diferente al que consiste primariamente de sonido grabado."@es,
        "Le son présent dans une ressource qui n’est pas constituée principalement de son enregistré."@fr ;
    rdakit:toolkitLabel "sound content"@en,
        "contenido sonoro"@es,
        "contenu sonore"@fr,
        "ljudinnehåll"@sv ;
    reg:hasUnconstrained <http://rdaregistry.info/Elements/u/P60559> ;
    reg:lexicalAlias <http://rdaregistry.info/Elements/e/soundContent.en> ;
    reg:name "soundContent"@en ;
    reg:status <http://metadataregistry.org/uri/RegStatus/1001> ;
    rdfs:domain <http://rdaregistry.info/Elements/c/C10006> ;
    rdfs:isDefinedBy <http://rdaregistry.info/Elements/e/> ;
    skos:definition "Relates an expression to a presence or absence of sound in an expression."@en .

<http://rdaregistry.info/Elements/e/P20229> a rdf:Property ;
    rdfs:label "has aspect ratio"@en ;
    rdakit:instructionNumber "7.19" ;
    rdakit:toolkitDefinition "A numerical ratio of the width to the height of a moving image."@en,
        "La relación de la anchura con la altura de una imagen móvil."@es,
        "Le rapport entre la largeur et la hauteur d’une image animée."@fr ;
    rdakit:toolkitLabel "aspect ratio"@en,
        "proporción dimensional"@es,
        "format de l’image"@fr ;
    reg:hasUnconstrained <http://rdaregistry.info/Elements/u/P60566> ;
    reg:lexicalAlias <http://rdaregistry.info/Elements/e/aspectRatioDesignation.en> ;
    reg:name "aspectRatio"@en ;
    reg:status <http://metadataregistry.org/uri/RegStatus/1001> ;
    rdfs:domain <http://rdaregistry.info/Elements/c/C10006> ;
    rdfs:isDefinedBy <http://rdaregistry.info/Elements/e/> ;
    skos:definition "Relates an expression to a numerical ratio of the width to the height of a moving image."@en .

<http://rdaregistry.info/Elements/e/P20231> a rdf:Property ;
    rdfs:label "has work expressed"@en,
        "har uttryckt verk"@sv ;
    rdakit:instructionNumber "17.6" ;
    rdakit:toolkitDefinition "A work realized through an expression."@en,
        "La obra realizada mediante una expresión"@es,
        "L’œuvre réalisée à travers une expression."@fr ;
    rdakit:toolkitLabel "work expressed"@en,
        "obra expresada"@es,
        "œuvre exprimée"@fr,
        "uttryckt verk"@sv ;
    reg:hasSubproperty <http://rdaregistry.info/Elements/e/object/P20231> ;
    reg:lexicalAlias <http://rdaregistry.info/Elements/e/workExpressed.en> ;
    reg:name "workExpressed"@en ;
    reg:status <http://metadataregistry.org/uri/RegStatus/1001> ;
    rdfs:domain <http://rdaregistry.info/Elements/c/C10006> ;
    rdfs:isDefinedBy <http://rdaregistry.info/Elements/e/> ;
    skos:definition "Relates an expression to a work realized through an expression."@en .

<http://rdaregistry.info/Elements/e/P20237> a rdf:Property ;
    rdfs:label "has writer of afterword"@en ;
    rdakit:instructionNumber "18.5" ;
    rdakit:toolkitDefinition "An agent contributing to an expression of a work by providing an afterword to an original work."@en,
        "Una persona, familia o entidad corporativa que contribuye a una expresión de una obra proporcionando un epílogo a la obra original."@es,
        "Personne, famille ou collectivité contribuant à une expression d’une œuvre en fournissant un après-propos à l’œuvre originale."@fr ;
    rdakit:toolkitLabel "writer of afterword"@en,
        "escritor de epílogo"@es,
        "auteur d’après-propos"@fr ;
    reg:hasSubproperty <http://rdaregistry.info/Elements/e/object/P20237> ;
    reg:hasUnconstrained <http://rdaregistry.info/Elements/u/P60715> ;
    reg:lexicalAlias <http://rdaregistry.info/Elements/e/writerOfAfterword.en> ;
    reg:name "writerOfAfterword"@en ;
    reg:status <http://metadataregistry.org/uri/RegStatus/1001> ;
    rdfs:domain <http://rdaregistry.info/Elements/c/C10006> ;
    rdfs:isDefinedBy <http://rdaregistry.info/Elements/e/> ;
    rdfs:subPropertyOf <http://rdaregistry.info/Elements/e/P20046> ;
    skos:definition "Relates an expression to an agent contributing to an expression of a work by providing an afterword to an original work."@en .

<http://rdaregistry.info/Elements/e/P20238> a rdf:Property ;
    rdfs:label "has writer of postface"@en ;
    rdakit:instructionNumber "18.5" ;
    rdakit:toolkitDefinition "An agent contributing to an expression of a work by providing a postface to an original work."@en,
        "Una persona, familia o entidad corporativa que contribuye a una expresión de una obra proporcionando unas palabras finales o conclusiones al original de la obra."@es,
        "Personne, famille ou collectivité contribuant à une expression d’une œuvre en fournissant une postface à l’œuvre originale."@fr ;
    rdakit:toolkitLabel "writer of postface"@en,
        "escritor de conclusión"@es,
        "postfacier"@fr ;
    reg:hasSubproperty <http://rdaregistry.info/Elements/e/object/P20238> ;
    reg:hasUnconstrained <http://rdaregistry.info/Elements/u/P60716> ;
    reg:lexicalAlias <http://rdaregistry.info/Elements/e/writerOfPostface.en> ;
    reg:name "writerOfPostface"@en ;
    reg:status <http://metadataregistry.org/uri/RegStatus/1001> ;
    rdfs:domain <http://rdaregistry.info/Elements/c/C10006> ;
    rdfs:isDefinedBy <http://rdaregistry.info/Elements/e/> ;
    rdfs:subPropertyOf <http://rdaregistry.info/Elements/e/P20046> ;
    skos:definition "Relates an expression to an agent contributing to an expression of a work by providing a postface to an original work."@en .

<http://rdaregistry.info/Elements/e/P20239> a rdf:Property ;
    rdfs:label "is musical theatre adaptation of (expression)"@en ;
    rdakit:instructionNumber "24.5" ;
    rdakit:toolkitDefinition "An expression of a work that has been adapted as a musical theatre work."@en,
        "Una expresión de una obra que ha sido adaptada como una obra de teatro musical."@es,
        "Expression d’une œuvre qui a été adaptée en œuvre de théâtre musical."@fr ;
    rdakit:toolkitLabel "musical theatre adaptation of (expression)"@en,
        "adaptación para teatro musical de (expresión)"@es,
        "adaptation au théâtre musical de (expression)"@fr ;
    reg:hasSubproperty <http://rdaregistry.info/Elements/e/object/P20239> ;
    reg:hasUnconstrained <http://rdaregistry.info/Elements/u/P60719> ;
    reg:lexicalAlias <http://rdaregistry.info/Elements/e/musicalTheatreAdaptationOfExpression.en> ;
    reg:name "musicalTheatreAdaptationOfExpression"@en ;
    reg:status <http://metadataregistry.org/uri/RegStatus/1001> ;
    rdfs:domain <http://rdaregistry.info/Elements/c/C10006> ;
    rdfs:isDefinedBy <http://rdaregistry.info/Elements/e/> ;
    rdfs:subPropertyOf <http://rdaregistry.info/Elements/e/P20152> ;
    skos:definition "Relates an expression to an expression of a work that has been adapted as a musical theatre work."@en .

<http://rdaregistry.info/Elements/e/P20240> a rdf:Property ;
    rdfs:label "is opera adaptation of (expression)"@en ;
    rdakit:instructionNumber "24.5" ;
    rdakit:toolkitDefinition "An expression of a work that has been adapted as an opera."@en,
        "Una expresión de una obra que ha sido adaptada como una ópera."@es,
        "Expression d’une œuvre qui a été adaptée à l’opéra."@fr ;
    rdakit:toolkitLabel "opera adaptation of (expression)"@en,
        "adaptación para ópera de (expresión)"@es,
        "adaptation à l’opéra de (expression)"@fr ;
    reg:hasSubproperty <http://rdaregistry.info/Elements/e/object/P20240> ;
    reg:hasUnconstrained <http://rdaregistry.info/Elements/u/P60720> ;
    reg:lexicalAlias <http://rdaregistry.info/Elements/e/operaAdaptationOfExpression.en> ;
    reg:name "operaAdaptationOfExpression"@en ;
    reg:status <http://metadataregistry.org/uri/RegStatus/1001> ;
    rdfs:domain <http://rdaregistry.info/Elements/c/C10006> ;
    rdfs:isDefinedBy <http://rdaregistry.info/Elements/e/> ;
    rdfs:subPropertyOf <http://rdaregistry.info/Elements/e/P20152> ;
    skos:definition "Relates an expression to an expression of a work that has been adapted as an opera."@en .

<http://rdaregistry.info/Elements/e/P20241> a rdf:Property ;
    rdfs:label "is adapted as musical theatre (expression)"@en ;
    rdakit:instructionNumber "24.5" ;
    rdakit:toolkitDefinition "An expression of a musical theatre work based on a source expression."@en,
        "Una expresión de una obra de teatro musical basada en la expresión fuente."@es,
        "Expression d’une œuvre de théâtre musical basée sur l’expression source."@fr ;
    rdakit:toolkitLabel "adapted as musical theatre (expression)"@en,
        "adaptada como teatro musical (expresión)"@es,
        "adapté au théâtre musical (expression)"@fr ;
    reg:hasSubproperty <http://rdaregistry.info/Elements/e/object/P20241> ;
    reg:hasUnconstrained <http://rdaregistry.info/Elements/u/P60721> ;
    reg:lexicalAlias <http://rdaregistry.info/Elements/e/adaptedAsMusicalTheatreExpression.en> ;
    reg:name "adaptedAsMusicalTheatreExpression"@en ;
    reg:status <http://metadataregistry.org/uri/RegStatus/1001> ;
    rdfs:domain <http://rdaregistry.info/Elements/c/C10006> ;
    rdfs:isDefinedBy <http://rdaregistry.info/Elements/e/> ;
    rdfs:subPropertyOf <http://rdaregistry.info/Elements/e/P20153> ;
    skos:definition "Relates an expression to an expression of a musical theatre work based on a source expression."@en .

<http://rdaregistry.info/Elements/e/P20242> a rdf:Property ;
    rdfs:label "is adapted as opera (expression)"@en ;
    rdakit:instructionNumber "24.5" ;
    rdakit:toolkitDefinition "An expression of an opera based on a source expression."@en,
        "Una expresión de una ópera basada en la expresión fuente."@es,
        "Expression d’un opéra basée sur l’expression source."@fr ;
    rdakit:toolkitLabel "adapted as opera (expression)"@en,
        "adaptada como ópera (expresión)"@es,
        "adapté en opéra"@fr ;
    reg:hasSubproperty <http://rdaregistry.info/Elements/e/object/P20242> ;
    reg:hasUnconstrained <http://rdaregistry.info/Elements/u/P60722> ;
    reg:lexicalAlias <http://rdaregistry.info/Elements/e/adaptedAsOperaExpression.en> ;
    reg:name "adaptedAsOperaExpression"@en ;
    reg:status <http://metadataregistry.org/uri/RegStatus/1001> ;
    rdfs:domain <http://rdaregistry.info/Elements/c/C10006> ;
    rdfs:isDefinedBy <http://rdaregistry.info/Elements/e/> ;
    rdfs:subPropertyOf <http://rdaregistry.info/Elements/e/P20153> ;
    skos:definition "Relates an expression to an expression of an opera based on a source expression."@en .

<http://rdaregistry.info/Elements/e/P20245> a rdf:Property ;
    rdfs:label "is video music (expression)"@en ;
    rdakit:instructionNumber "24.5" ;
    rdakit:toolkitDefinition "An expression of a musical work that is used in a video."@en,
        "Una expresión de una obra musical que es usada en un video."@es,
        "Expression d’une œuvre musicale utilisée dans une vidéo."@fr ;
    rdakit:toolkitLabel "video music (expression)"@en,
        "música de video (expresión)"@es,
        "musique de vidéo (expression)"@fr ;
    reg:hasSubproperty <http://rdaregistry.info/Elements/e/object/P20245> ;
    reg:hasUnconstrained <http://rdaregistry.info/Elements/u/P60725> ;
    reg:lexicalAlias <http://rdaregistry.info/Elements/e/videoMusicExpression.en> ;
    reg:name "videoMusicExpression"@en ;
    reg:status <http://metadataregistry.org/uri/RegStatus/1001> ;
    rdfs:domain <http://rdaregistry.info/Elements/c/C10006> ;
    rdfs:isDefinedBy <http://rdaregistry.info/Elements/e/> ;
    rdfs:subPropertyOf <http://rdaregistry.info/Elements/e/P20243> ;
    skos:definition "Relates an expression to an expression of a musical work that is used in a video."@en .

<http://rdaregistry.info/Elements/e/P20246> a rdf:Property ;
    rdfs:label "is music for video (expression)"@en ;
    rdakit:instructionNumber "24.5" ;
    rdakit:toolkitDefinition "An expression of a work that uses a musical work in a video."@en,
        "Una expresión de una obra que usa la obra musical en un video"@es,
        "Expression d’une œuvre qui utilise l’œuvre musicale dans une vidéo."@fr ;
    rdakit:toolkitLabel "music for video (expression)"@en,
        "música para video (expresión)"@es,
        "musique pour la vidéo (expression)"@fr ;
    reg:hasSubproperty <http://rdaregistry.info/Elements/e/object/P20246> ;
    reg:hasUnconstrained <http://rdaregistry.info/Elements/u/P60726> ;
    reg:lexicalAlias <http://rdaregistry.info/Elements/e/musicForVideoExpression.en> ;
    reg:name "musicForVideoExpression"@en ;
    reg:status <http://metadataregistry.org/uri/RegStatus/1001> ;
    rdfs:domain <http://rdaregistry.info/Elements/c/C10006> ;
    rdfs:isDefinedBy <http://rdaregistry.info/Elements/e/> ;
    rdfs:subPropertyOf <http://rdaregistry.info/Elements/e/P20244> ;
    skos:definition "Relates an expression to an expression of a work that uses a musical work in a video."@en .

<http://rdaregistry.info/Elements/e/P20247> a rdf:Property ;
    rdfs:label "is television program music (expression)"@en ;
    rdakit:instructionNumber "24.5" ;
    rdakit:toolkitDefinition "An expression of a musical work that is used in a television program."@en,
        "Una expresión de una obra musical que es usada en un programa de televisión."@es,
        "Expression d’une œuvre musicale utilisée dans une émission de télévision."@fr ;
    rdakit:toolkitLabel "television program music (expression)"@en,
        "música de programa de televisión (expresión)"@es,
        "musique d’émission de télévision (expression)"@fr ;
    reg:hasSubproperty <http://rdaregistry.info/Elements/e/object/P20247> ;
    reg:hasUnconstrained <http://rdaregistry.info/Elements/u/P60727> ;
    reg:lexicalAlias <http://rdaregistry.info/Elements/e/televisionProgramMusicExpression.en> ;
    reg:name "televisionProgramMusicExpression"@en ;
    reg:status <http://metadataregistry.org/uri/RegStatus/1001> ;
    rdfs:domain <http://rdaregistry.info/Elements/c/C10006> ;
    rdfs:isDefinedBy <http://rdaregistry.info/Elements/e/> ;
    rdfs:subPropertyOf <http://rdaregistry.info/Elements/e/P20243> ;
    skos:definition "Relates an expression to an expression of a musical work that is used in a television program."@en .

<http://rdaregistry.info/Elements/e/P20248> a rdf:Property ;
    rdfs:label "is music for television program (expression)"@en ;
    rdakit:instructionNumber "24.5" ;
    rdakit:toolkitDefinition "An expression of a work that uses a musical work in a television program."@en,
        "Una expresión de una obra que usa la obra musical en un programa de televisión."@es,
        "Expression d’une œuvre qui utilise l’œuvre musicale dans une émission de télévision."@fr ;
    rdakit:toolkitLabel "music for television program (expression)"@en,
        "música para programa de televisión (expresión)"@es,
        "musique pour l’émission de télévision (expression)"@fr ;
    reg:hasSubproperty <http://rdaregistry.info/Elements/e/object/P20248> ;
    reg:hasUnconstrained <http://rdaregistry.info/Elements/u/P60728> ;
    reg:lexicalAlias <http://rdaregistry.info/Elements/e/musicForTelevisionProgramExpression.en> ;
    reg:name "musicForTelevisionProgramExpression"@en ;
    reg:status <http://metadataregistry.org/uri/RegStatus/1001> ;
    rdfs:domain <http://rdaregistry.info/Elements/c/C10006> ;
    rdfs:isDefinedBy <http://rdaregistry.info/Elements/e/> ;
    rdfs:subPropertyOf <http://rdaregistry.info/Elements/e/P20244> ;
    skos:definition "Relates an expression to an expression of a work that uses a musical work in a television program."@en .

<http://rdaregistry.info/Elements/e/P20249> a rdf:Property ;
    rdfs:label "is radio program music (expression)"@en ;
    rdakit:instructionNumber "24.5" ;
    rdakit:toolkitDefinition "An expression of a musical work that is used in a radio program."@en,
        "Una expresión de una obra musical que es usada en un programa radiofónico."@es,
        "Expression d’une œuvre musicale utilisée dans une émission de radio."@fr ;
    rdakit:toolkitLabel "radio program music (expression)"@en,
        "música de programa radiofónico (expresión)"@es,
        "musique d’émission de radio (expression)"@fr ;
    reg:hasSubproperty <http://rdaregistry.info/Elements/e/object/P20249> ;
    reg:hasUnconstrained <http://rdaregistry.info/Elements/u/P60729> ;
    reg:lexicalAlias <http://rdaregistry.info/Elements/e/radioProgramMusicExpression.en> ;
    reg:name "radioProgramMusicExpression"@en ;
    reg:status <http://metadataregistry.org/uri/RegStatus/1001> ;
    rdfs:domain <http://rdaregistry.info/Elements/c/C10006> ;
    rdfs:isDefinedBy <http://rdaregistry.info/Elements/e/> ;
    rdfs:subPropertyOf <http://rdaregistry.info/Elements/e/P20243> ;
    skos:definition "Relates an expression to an expression of a musical work that is used in a radio program."@en .

<http://rdaregistry.info/Elements/e/P20250> a rdf:Property ;
    rdfs:label "is music for radio program (expression)"@en ;
    rdakit:instructionNumber "24.5" ;
    rdakit:toolkitDefinition "An expression of a work that uses a musical work in a radio program."@en,
        "Una expresión de una obra que usa la obra musical en un programa radiofónico."@es,
        "Expression d’une œuvre qui utilise l’œuvre musicale dans une émission de radio."@fr ;
    rdakit:toolkitLabel "music for radio program (expression)"@en,
        "música para programa radiofónico (expresión)"@es,
        "musique pour l’émission de radio (expression)"@fr ;
    reg:hasSubproperty <http://rdaregistry.info/Elements/e/object/P20250> ;
    reg:hasUnconstrained <http://rdaregistry.info/Elements/u/P60730> ;
    reg:lexicalAlias <http://rdaregistry.info/Elements/e/musicForRadioProgramExpression.en> ;
    reg:name "musicForRadioProgramExpression"@en ;
    reg:status <http://metadataregistry.org/uri/RegStatus/1001> ;
    rdfs:domain <http://rdaregistry.info/Elements/c/C10006> ;
    rdfs:isDefinedBy <http://rdaregistry.info/Elements/e/> ;
    rdfs:subPropertyOf <http://rdaregistry.info/Elements/e/P20244> ;
    skos:definition "Relates an expression to an expression of a work that uses a musical work in a radio program."@en .

<http://rdaregistry.info/Elements/e/P20251> a rdf:Property ;
    rdfs:label "is motion picture music (expression)"@en ;
    rdakit:instructionNumber "24.5" ;
    rdakit:toolkitDefinition "An expression of a musical work that is used in a motion picture."@en,
        "Una expresión de una obra musical que es usada en una película cinematográfica."@es,
        "Expression d’une œuvre musicale utilisée dans un film."@fr ;
    rdakit:toolkitLabel "motion picture music (expression)"@en,
        "música de película cinematográfica (expresión)"@es,
        "musique de film (expression)"@fr ;
    reg:hasSubproperty <http://rdaregistry.info/Elements/e/object/P20251> ;
    reg:hasUnconstrained <http://rdaregistry.info/Elements/u/P60731> ;
    reg:lexicalAlias <http://rdaregistry.info/Elements/e/motionPictureMusicExpression.en> ;
    reg:name "motionPictureMusicExpression"@en ;
    reg:status <http://metadataregistry.org/uri/RegStatus/1001> ;
    rdfs:domain <http://rdaregistry.info/Elements/c/C10006> ;
    rdfs:isDefinedBy <http://rdaregistry.info/Elements/e/> ;
    rdfs:subPropertyOf <http://rdaregistry.info/Elements/e/P20243> ;
    skos:definition "Relates an expression to an expression of a musical work that is used in a motion picture."@en .

<http://rdaregistry.info/Elements/e/P20252> a rdf:Property ;
    rdfs:label "is music for motion picture (expression)"@en ;
    rdakit:instructionNumber "24.5" ;
    rdakit:toolkitDefinition "An expression of a work that uses a musical work in a motion picture."@en,
        "Una expresión de una obra que usa la obra musical en una película cinematográfica."@es,
        "Expression d’une œuvre qui utilise l’œuvre musicale dans un film."@fr ;
    rdakit:toolkitLabel "music for motion picture (expression)"@en,
        "música para película cinematográfica (expresión)"@es,
        "musique pour le film (expression)"@fr ;
    reg:hasSubproperty <http://rdaregistry.info/Elements/e/object/P20252> ;
    reg:hasUnconstrained <http://rdaregistry.info/Elements/u/P60732> ;
    reg:lexicalAlias <http://rdaregistry.info/Elements/e/musicForMotionPictureExpression.en> ;
    reg:name "musicForMotionPictureExpression"@en ;
    reg:status <http://metadataregistry.org/uri/RegStatus/1001> ;
    rdfs:domain <http://rdaregistry.info/Elements/c/C10006> ;
    rdfs:isDefinedBy <http://rdaregistry.info/Elements/e/> ;
    rdfs:subPropertyOf <http://rdaregistry.info/Elements/e/P20244> ;
    skos:definition "Relates an expression to an expression of a work that uses a musical work in a motion picture."@en .

<http://rdaregistry.info/Elements/e/P20260> a rdf:Property ;
    rdfs:label "has details of aspect ratio designation"@en ;
    rdakit:instructionNumber "7.19.1.4.1.4" ;
    rdakit:toolkitDefinition "Details of the ratio of the width to the height of a moving image."@en,
        "Detalles de la relación de la anchura con la altura de una imagen móvil."@es ;
    rdakit:toolkitLabel "details of aspect ratio designation"@en,
        "detalles de la proporción dimensional"@es ;
    reg:hasUnconstrained <http://rdaregistry.info/Elements/u/P60760> ;
    reg:lexicalAlias <http://rdaregistry.info/Elements/e/detailsOfAspectRatioDesignation.en> ;
    reg:name "detailsOfAspectRatioDesignation"@en ;
    reg:status <http://metadataregistry.org/uri/RegStatus/1001> ;
    rdfs:domain <http://rdaregistry.info/Elements/c/C10006> ;
    rdfs:isDefinedBy <http://rdaregistry.info/Elements/e/> ;
    skos:definition "Relates an expression to details of the ratio of the width to the height of a moving image."@en .

<http://rdaregistry.info/Elements/e/P20261> a rdf:Property ;
    rdfs:label "has details of colour content"@en,
        "har detaljerad information om färginnehåll"@sv ;
    rdakit:instructionNumber "7.17.1.4" ;
    rdakit:toolkitDefinition "Details of the presence of colour, tone, etc., in the content of an expression, and the specific colours, tones, etc., including black and white, present."@en,
        "Detalles de la presencia de color, tono, etc., y los colores específicos, tonos, etc. (incluyendo blanco y negro) presentes en el contenido de un recurso."@es ;
    rdakit:toolkitLabel "details of colour content"@en,
        "detalles del contenido a color"@es,
        "detaljerad information om färginnehåll"@sv ;
    reg:hasUnconstrained <http://rdaregistry.info/Elements/u/P60761> ;
    reg:lexicalAlias <http://rdaregistry.info/Elements/e/detailsOfColourContent.en> ;
    reg:name "detailsOfColourContent"@en ;
    reg:status <http://metadataregistry.org/uri/RegStatus/1001> ;
    rdfs:domain <http://rdaregistry.info/Elements/c/C10006> ;
    rdfs:isDefinedBy <http://rdaregistry.info/Elements/e/> ;
    skos:definition "Relates an expression to details of the presence of colour, tone, etc., in the content of an expression, and the specific colours, tones, etc., including black and white, present."@en .

<http://rdaregistry.info/Elements/e/P20262> a rdf:Property ;
    rdfs:label "has details of form of musical notation"@en,
        "har detaljerad information om form av musiknotation"@sv ;
    rdakit:instructionNumber "7.13.3.4" ;
    rdakit:toolkitDefinition "Details of the set of characters or symbols used to express musical content of an expression."@en,
        "Detalles del conjunto de caracteres y/o símbolos utilizados para expresar el contenido musical de un recurso."@es ;
    rdakit:toolkitLabel "details of form of musical notation"@en,
        "detalles de la forma de la notación musical"@es,
        "detaljerad information om form av musiknotation"@sv ;
    reg:hasUnconstrained <http://rdaregistry.info/Elements/u/P60762> ;
    reg:lexicalAlias <http://rdaregistry.info/Elements/e/detailsOfFormOfMusicalNotation.en> ;
    reg:name "detailsOfFormOfMusicalNotation"@en ;
    reg:status <http://metadataregistry.org/uri/RegStatus/1001> ;
    rdfs:domain <http://rdaregistry.info/Elements/c/C10006> ;
    rdfs:isDefinedBy <http://rdaregistry.info/Elements/e/> ;
    skos:definition "Relates an expression to details of a set of characters or symbols used to express musical content of an expression."@en,
        "Relates an expression to details of the set of characters or symbols used to express musical content of an expression."@en .

<http://rdaregistry.info/Elements/e/P20263> a rdf:Property ;
    rdfs:label "has details of form of notated movement"@en,
        "har detaljerad information om form av noterad rörelse"@sv ;
    rdakit:instructionNumber "7.13.5.4" ;
    rdakit:toolkitDefinition "Details of the set of characters or symbols used to express movement content of an expression."@en,
        "Detalles del conjunto de caracteres y/o símbolos usados para expresar el contenido de movimientos de un recurso."@es ;
    rdakit:toolkitLabel "details of form of notated movement"@en,
        "detalles de la forma de notación de movimientos"@es,
        "detaljerad information om form av noterad rörelse"@sv ;
    reg:hasUnconstrained <http://rdaregistry.info/Elements/u/P60763> ;
    reg:lexicalAlias <http://rdaregistry.info/Elements/e/detailsOfFormOfNotatedMovement.en> ;
    reg:name "detailsOfFormOfNotatedMovement"@en ;
    reg:status <http://metadataregistry.org/uri/RegStatus/1001> ;
    rdfs:domain <http://rdaregistry.info/Elements/c/C10006> ;
    rdfs:isDefinedBy <http://rdaregistry.info/Elements/e/> ;
    skos:definition "Relates an expression to details of a set of characters or symbols used to express movement content of an expression."@en,
        "Relates an expression to details of the set of characters or symbols used to express movement content of an expression."@en .

<http://rdaregistry.info/Elements/e/P20264> a rdf:Property ;
    rdfs:label "has details of format of notated music"@en,
        "har detaljerad information om format för noterad musik"@sv ;
    rdakit:instructionNumber "7.20.1.4" ;
    rdakit:toolkitDefinition "Details of the musical or physical layout of the content of an expression that is presented in the form of musical notation."@en,
        "Detalles de la presentación musical o física del contenido de un recurso que se presenta en forma de notación musical."@es ;
    rdakit:toolkitLabel "details of format of notated music"@en,
        "detalles del formato de la música notada"@es,
        "detaljerad information om format för noterad musik"@sv ;
    reg:hasUnconstrained <http://rdaregistry.info/Elements/u/P60764> ;
    reg:lexicalAlias <http://rdaregistry.info/Elements/e/detailsOfFormatOfNotatedMusic.en> ;
    reg:name "detailsOfFormatOfNotatedMusic"@en ;
    reg:status <http://metadataregistry.org/uri/RegStatus/1001> ;
    rdfs:domain <http://rdaregistry.info/Elements/c/C10006> ;
    rdfs:isDefinedBy <http://rdaregistry.info/Elements/e/> ;
    skos:definition "Relates an expression to details of the musical or physical layout of the content of an expression that is presented in the form of musical notation."@en .

<http://rdaregistry.info/Elements/e/P20265> a rdf:Property ;
    rdfs:label "has details of form of tactile notation"@en,
        "har detaljerad information om form av taktil notation"@sv ;
    rdakit:instructionNumber "7.13.4.4" ;
    rdakit:toolkitDefinition "Details of the set of characters or symbols used to express the content of an expression in a form that can be perceived through touch."@en,
        "Detalles del conjunto de caracteres y/o símbolos utilizados para expresar el contenido de un recurso en tal forma que se pueda percibir mediante el tacto."@es ;
    rdakit:toolkitLabel "details of form of tactile notation"@en,
        "detalles de la forma de la notación táctil"@es,
        "detaljerad information om form av taktil notation"@sv ;
    reg:hasUnconstrained <http://rdaregistry.info/Elements/u/P60765> ;
    reg:lexicalAlias <http://rdaregistry.info/Elements/e/detailsOfFormOfTactileNotation.en> ;
    reg:name "detailsOfFormOfTactileNotation"@en ;
    reg:status <http://metadataregistry.org/uri/RegStatus/1001> ;
    rdfs:domain <http://rdaregistry.info/Elements/c/C10006> ;
    rdfs:isDefinedBy <http://rdaregistry.info/Elements/e/> ;
    skos:definition "Relates an expression to details of a set of characters or symbols used to express the content of an expression in a form that can be perceived through touch."@en,
        "Relates an expression to details of the set of characters or symbols used to express the content of an expression in a form that can be perceived through touch."@en .

<http://rdaregistry.info/Elements/e/P20266> a rdf:Property ;
    rdfs:label "has details of script"@en,
        "har detaljerad information om skriftart"@sv ;
    rdakit:instructionNumber "7.13.2.4" ;
    rdakit:toolkitDefinition "Details of the set of characters or symbols used to express written language content of an expression."@en,
        "Detalles del conjunto de caracteres y/o símbolos usados para expresar el contenido de lengua escrita de un recurso."@es ;
    rdakit:toolkitLabel "details of script"@en,
        "detalles de la escritura"@es,
        "detaljerad information om skriftart"@sv ;
    reg:hasUnconstrained <http://rdaregistry.info/Elements/u/P60766> ;
    reg:lexicalAlias <http://rdaregistry.info/Elements/e/detailsOfScript.en> ;
    reg:name "detailsOfScript"@en ;
    reg:status <http://metadataregistry.org/uri/RegStatus/1001> ;
    rdfs:domain <http://rdaregistry.info/Elements/c/C10006> ;
    rdfs:isDefinedBy <http://rdaregistry.info/Elements/e/> ;
    skos:definition "Relates an expression to details of a set of characters or symbols used to express written language content of an expression."@en,
        "Relates an expression to details of the set of characters or symbols used to express written language content of an expression."@en .

<http://rdaregistry.info/Elements/e/P20267> a rdf:Property ;
    rdfs:label "has details of illustrative content"@en,
        "har detaljerad information om illustrativt innehåll"@sv ;
    rdakit:instructionNumber "7.15.1.4" ;
    rdakit:toolkitDefinition "Details of content intended to illustrate the primary content of an expression."@en,
        "Detalles del contenido destinado a ilustrar el contenido primario de un recurso."@es ;
    rdakit:toolkitLabel "details of illustrative content"@en,
        "detalles del contenido ilustrativo"@es,
        "detaljerad information om illustrativt innehåll"@sv ;
    reg:hasUnconstrained <http://rdaregistry.info/Elements/u/P60804> ;
    reg:lexicalAlias <http://rdaregistry.info/Elements/e/detailsOfIllustrativeContent.en> ;
    reg:name "detailsOfIllustrativeContent"@en ;
    reg:status <http://metadataregistry.org/uri/RegStatus/1001> ;
    rdfs:domain <http://rdaregistry.info/Elements/c/C10006> ;
    rdfs:isDefinedBy <http://rdaregistry.info/Elements/e/> ;
    skos:definition "Relates an expression to details of content intended to illustrate the primary content of an expression."@en .

<http://rdaregistry.info/Elements/e/P20278> a rdf:Property ;
    rdfs:label "has details of duration"@en,
        "har detaljerad information om speltid"@sv ;
    rdakit:instructionNumber "7.22.1.5" ;
    rdakit:toolkitDefinition "Details of a playing time, running time, performance time, etc., of the content of an expression."@en,
        "Tiempo de reproducción, duración, interpretación, etc., del contenido de un recurso."@es ;
    rdakit:toolkitLabel "details of duration"@en,
        "detalles de duración"@es,
        "detaljerad information om speltid"@sv ;
    reg:hasUnconstrained <http://rdaregistry.info/Elements/u/P60823> ;
    reg:lexicalAlias <http://rdaregistry.info/Elements/e/detailsOfDuration.en> ;
    reg:name "detailsOfDuration"@en ;
    reg:status <http://metadataregistry.org/uri/RegStatus/1001> ;
    rdfs:domain <http://rdaregistry.info/Elements/c/C10006> ;
    rdfs:isDefinedBy <http://rdaregistry.info/Elements/e/> ;
    skos:definition "Relates an expression to details of a playing time, running time, performance time, etc., of the content of an expression."@en .

<http://rdaregistry.info/Elements/e/P20290> a rdf:Property ;
    rdfs:label "has aspect ratio designation"@en ;
    rdakit:instructionNumber "7.19.1.4" ;
    rdakit:toolkitDefinition "A general designation of the ratio of the width to the height of a moving image."@en ;
    rdakit:toolkitLabel "aspect ratio designation"@en ;
    reg:hasUnconstrained <http://rdaregistry.info/Elements/u/P60873> ;
    reg:lexicalAlias <http://rdaregistry.info/Elements/e/aspectRatioDesignation.en> ;
    reg:name "aspectRatioDesignation"@en ;
    reg:status <http://metadataregistry.org/uri/RegStatus/1001> ;
    rdfs:domain <http://rdaregistry.info/Elements/c/C10006> ;
    rdfs:isDefinedBy <http://rdaregistry.info/Elements/e/> ;
    skos:definition "Relates an expression to a general designation of the ratio of the width to the height of a moving image."@en .

<http://rdaregistry.info/Elements/e/P20291> a rdf:Property ;
    rdfs:label "has scale designation"@en ;
    rdakit:instructionNumber "7.25.6" ;
    rdakit:toolkitDefinition "A general designation of the lack of a ratio of the dimensions of the content of an image or three-dimensional form to the dimensions of the thing that is represented."@en ;
    rdakit:toolkitLabel "scale designation"@en ;
    reg:hasUnconstrained <http://rdaregistry.info/Elements/u/P60874> ;
    reg:lexicalAlias <http://rdaregistry.info/Elements/e/scaleDesignation.en> ;
    reg:name "scaleDesignation"@en ;
    reg:status <http://metadataregistry.org/uri/RegStatus/1001> ;
    rdfs:domain <http://rdaregistry.info/Elements/c/C10006> ;
    rdfs:isDefinedBy <http://rdaregistry.info/Elements/e/> ;
    skos:definition "Relates an expression to a general designation of the lack of a ratio of the dimensions of the content of an image or three-dimensional form to the dimensions of the thing that is represented."@en .

<http://rdaregistry.info/Elements/e/P20298> a rdf:Property ;
    rdfs:label "has related work (expression)"@en ;
    reg:hasSubproperty <http://rdaregistry.info/Elements/e/datatype/P20298>,
        <http://rdaregistry.info/Elements/e/object/P20298> ;
    reg:hasUnconstrained <http://rdaregistry.info/Elements/u/P60313> ;
    reg:lexicalAlias <http://rdaregistry.info/Elements/e/relatedWorkExpression.en> ;
    reg:name "relatedWorkExpression"@en ;
    reg:status <http://metadataregistry.org/uri/RegStatus/1001> ;
    rdfs:domain <http://rdaregistry.info/Elements/c/C10006> ;
    rdfs:isDefinedBy <http://rdaregistry.info/Elements/e/> ;
    rdfs:subPropertyOf <http://rdaregistry.info/Elements/e/P20297> ;
    skos:definition "Relates an expression to a work associated with an expression being described."@en .

<http://rdaregistry.info/Elements/e/P20299> a rdf:Property ;
    rdfs:label "has related manifestation (expression)"@en ;
    reg:hasSubproperty <http://rdaregistry.info/Elements/e/datatype/P20299>,
        <http://rdaregistry.info/Elements/e/object/P20299> ;
    reg:hasUnconstrained <http://rdaregistry.info/Elements/u/P60313> ;
    reg:lexicalAlias <http://rdaregistry.info/Elements/e/relatedManifestationExpression.en> ;
    reg:name "relatedManifestationExpression"@en ;
    reg:status <http://metadataregistry.org/uri/RegStatus/1001> ;
    rdfs:domain <http://rdaregistry.info/Elements/c/C10006> ;
    rdfs:isDefinedBy <http://rdaregistry.info/Elements/e/> ;
    rdfs:subPropertyOf <http://rdaregistry.info/Elements/e/P20297> ;
    skos:definition "Relates an expression to a manifestation associated with an expression being described."@en .

<http://rdaregistry.info/Elements/e/P20300> a rdf:Property ;
    rdfs:label "has related item (expression)"@en ;
    reg:hasSubproperty <http://rdaregistry.info/Elements/e/datatype/P20300>,
        <http://rdaregistry.info/Elements/e/object/P20300> ;
    reg:hasUnconstrained <http://rdaregistry.info/Elements/u/P60313> ;
    reg:lexicalAlias <http://rdaregistry.info/Elements/e/relatedItemExpression.en> ;
    reg:name "relatedItemExpression"@en ;
    reg:status <http://metadataregistry.org/uri/RegStatus/1001> ;
    rdfs:domain <http://rdaregistry.info/Elements/c/C10006> ;
    rdfs:isDefinedBy <http://rdaregistry.info/Elements/e/> ;
    rdfs:subPropertyOf <http://rdaregistry.info/Elements/e/P20297> ;
    skos:definition "Relates an expression to an item associated with an expression being described."@en .

<http://rdaregistry.info/Elements/e/P20302> a rdf:Property ;
    rdfs:label "has related person (expression)"@en ;
    reg:hasSubproperty <http://rdaregistry.info/Elements/e/datatype/P20302>,
        <http://rdaregistry.info/Elements/e/object/P20302> ;
    reg:lexicalAlias <http://rdaregistry.info/Elements/e/relatedPersonExpression.en> ;
    reg:name "relatedPersonExpression"@en ;
    reg:status <http://metadataregistry.org/uri/RegStatus/1001> ;
    rdfs:domain <http://rdaregistry.info/Elements/c/C10006> ;
    rdfs:isDefinedBy <http://rdaregistry.info/Elements/e/> ;
    rdfs:subPropertyOf <http://rdaregistry.info/Elements/e/P20301> ;
    skos:definition "Relates an expression to a person associated with an expression being described."@en .

<http://rdaregistry.info/Elements/e/P20303> a rdf:Property ;
    rdfs:label "has related family (expression)"@en ;
    reg:hasSubproperty <http://rdaregistry.info/Elements/e/datatype/P20303>,
        <http://rdaregistry.info/Elements/e/object/P20303> ;
    reg:lexicalAlias <http://rdaregistry.info/Elements/e/relatedFamilyExpression.en> ;
    reg:name "relatedFamilyExpression"@en ;
    reg:status <http://metadataregistry.org/uri/RegStatus/1001> ;
    rdfs:domain <http://rdaregistry.info/Elements/c/C10006> ;
    rdfs:isDefinedBy <http://rdaregistry.info/Elements/e/> ;
    rdfs:subPropertyOf <http://rdaregistry.info/Elements/e/P20305> ;
    skos:definition "Relates an expression to a family associated with an expression being described."@en .

<http://rdaregistry.info/Elements/e/P20304> a rdf:Property ;
    rdfs:label "has related corporate body (expression)"@en ;
    reg:hasSubproperty <http://rdaregistry.info/Elements/e/datatype/P20304>,
        <http://rdaregistry.info/Elements/e/object/P20304> ;
    reg:lexicalAlias <http://rdaregistry.info/Elements/e/relatedCorporateBodyExpression.en> ;
    reg:name "relatedCorporateBodyExpression"@en ;
    reg:status <http://metadataregistry.org/uri/RegStatus/1001> ;
    rdfs:domain <http://rdaregistry.info/Elements/c/C10006> ;
    rdfs:isDefinedBy <http://rdaregistry.info/Elements/e/> ;
    rdfs:subPropertyOf <http://rdaregistry.info/Elements/e/P20305> ;
    skos:definition "Relates an expression to a corporate body associated with an expression being described."@en .

<http://rdaregistry.info/Elements/e/P20306> a rdf:Property ;
    rdfs:label "has related place (expression)"@en ;
    reg:hasSubproperty <http://rdaregistry.info/Elements/e/datatype/P20306>,
        <http://rdaregistry.info/Elements/e/object/P20306> ;
    reg:lexicalAlias <http://rdaregistry.info/Elements/e/relatedPlaceExpression.en> ;
    reg:name "relatedPlaceExpression"@en ;
    reg:status <http://metadataregistry.org/uri/RegStatus/1001> ;
    rdfs:domain <http://rdaregistry.info/Elements/c/C10006> ;
    rdfs:isDefinedBy <http://rdaregistry.info/Elements/e/> ;
    rdfs:subPropertyOf <http://rdaregistry.info/Elements/e/P20297> ;
    skos:definition "Relates an expression to a place associated with an expression being described."@en .

<http://rdaregistry.info/Elements/e/P20307> a rdf:Property ;
    rdfs:label "has related time-span (expression)"@en ;
    reg:hasSubproperty <http://rdaregistry.info/Elements/e/datatype/P20307>,
        <http://rdaregistry.info/Elements/e/object/P20307> ;
    reg:lexicalAlias <http://rdaregistry.info/Elements/e/relatetdTimespanExpression.en> ;
    reg:name "relatetdTimespanExpression"@en ;
    reg:status <http://metadataregistry.org/uri/RegStatus/1001> ;
    rdfs:domain <http://rdaregistry.info/Elements/c/C10006> ;
    rdfs:isDefinedBy <http://rdaregistry.info/Elements/e/> ;
    rdfs:subPropertyOf <http://rdaregistry.info/Elements/e/P20297> ;
    skos:definition "Relates an expression to a time-span associated with an expression being described."@en .

<http://rdaregistry.info/Elements/e/P20308> a rdf:Property ;
    rdfs:label "has related nomen (expression)"@en ;
    reg:hasSubproperty <http://rdaregistry.info/Elements/e/datatype/P20308>,
        <http://rdaregistry.info/Elements/e/object/P20308> ;
    reg:lexicalAlias <http://rdaregistry.info/Elements/e/relatedNomenExpression.en> ;
    reg:name "relatedNomenExpression"@en ;
    reg:status <http://metadataregistry.org/uri/RegStatus/1001> ;
    rdfs:domain <http://rdaregistry.info/Elements/c/C10006> ;
    rdfs:isDefinedBy <http://rdaregistry.info/Elements/e/> ;
    rdfs:subPropertyOf <http://rdaregistry.info/Elements/e/P20297> ;
    skos:definition "Relates an expression to a nomen associated with an expression being described."@en .

<http://rdaregistry.info/Elements/e/P20309> a rdf:Property ;
    rdfs:label "has note on capture"@en ;
    rdakit:instructionNumber "7.11.4" ;
    rdakit:toolkitDefinition "A note providing information associated with the recording, filming, etc., of the content of an expression."@en ;
    rdakit:toolkitLabel "note on capture"@en ;
    reg:hasUnconstrained <http://rdaregistry.info/Elements/u/P60905> ;
    reg:lexicalAlias <http://rdaregistry.info/Elements/e/noteOnCapture.en> ;
    reg:name "noteOnCapture"@en ;
    reg:status <http://metadataregistry.org/uri/RegStatus/1001> ;
    rdfs:domain <http://rdaregistry.info/Elements/c/C10006> ;
    rdfs:isDefinedBy <http://rdaregistry.info/Elements/e/> ;
    rdfs:subPropertyOf <http://rdaregistry.info/Elements/e/P20071> ;
    skos:definition "Relates an expression to a note providing information associated with the recording, filming, etc., of the content of an expression."@en ;
    skos:scopeNote "Note on capture includes the circumstances such as a live or studio recording, the equipment used, etc."@en .

<http://rdaregistry.info/Elements/e/P20007> a rdf:Property ;
    rdfs:label "has language of content"@en ;
    rdakit:instructionNumber "7.12" ;
    rdakit:toolkitDefinition "A language used to express the content of an expression."@en,
        "Una lengua utilizada para expresar el contenido de un recurso."@es,
        "Langue utilisée pour exprimer le contenu d’une ressource."@fr ;
    rdakit:toolkitLabel "language of content"@en,
        "lengua del contenido"@es,
        "langue du contenu"@fr ;
    reg:hasUnconstrained <http://rdaregistry.info/Elements/u/P60099> ;
    reg:lexicalAlias <http://rdaregistry.info/Elements/e/languageOfContent.en> ;
    reg:name "languageOfContent"@en ;
    reg:status <http://metadataregistry.org/uri/RegStatus/1001> ;
    rdfs:domain <http://rdaregistry.info/Elements/c/C10006> ;
    rdfs:isDefinedBy <http://rdaregistry.info/Elements/e/> ;
    skos:definition "Relates an expression to a language used to express the content of an expression."@en .

<http://rdaregistry.info/Elements/e/P20009> a rdf:Property ;
    rdfs:label "is adapted as motion picture (expression)"@en ;
    rdakit:instructionNumber "24.5" ;
    rdakit:toolkitDefinition "A motion picture based on a source expression."@en,
        "Una película cinematográfica basada en la expresión fuente."@es,
        "Film basé sur l’expression source."@fr ;
    rdakit:toolkitLabel "adapted as motion picture (expression)"@en,
        "adaptada como película cinematográfica (expresión)"@es,
        "adapté en film (expression)"@fr ;
    reg:hasSubproperty <http://rdaregistry.info/Elements/e/object/P20009> ;
    reg:hasUnconstrained <http://rdaregistry.info/Elements/u/P60110> ;
    reg:lexicalAlias <http://rdaregistry.info/Elements/e/adaptedAsMotionPictureExpression.en> ;
    reg:name "adaptedAsMotionPictureExpression"@en ;
    reg:status <http://metadataregistry.org/uri/RegStatus/1001> ;
    rdfs:domain <http://rdaregistry.info/Elements/c/C10006> ;
    rdfs:isDefinedBy <http://rdaregistry.info/Elements/e/> ;
    rdfs:subPropertyOf <http://rdaregistry.info/Elements/e/P20153> ;
    skos:definition "Relates an expression to a motion picture based on a source expression."@en .

<http://rdaregistry.info/Elements/e/P20010> a rdf:Property ;
    rdfs:label "has note on changes in content characteristics"@en,
        "har anmärkning om förändringar i innehållsegenskaper"@sv ;
    rdakit:instructionNumber "7.29.2" ;
    rdakit:toolkitDefinition "A note on changes in content characteristics that occur in subsequent issues or parts of an expression issued in successive parts or between iterations of an integrating resource."@en,
        "Una nota sobre cambios en las características que ocurren en entregas o partes subsecuentes de un recurso publicado en partes sucesivas o entre iteraciones de un recurso integrable."@es,
        "Note portant sur les changements de caractéristiques du contenu survenant dans les livraisons ou les parties ultérieures d’une ressource publiée en parties successives ou bien entre les différentes itérations d’une ressource intégratrice."@fr ;
    rdakit:toolkitLabel "note on changes in content characteristics"@en,
        "nota sobre cambios en las características del contenido"@es,
        "note relative aux changements de caractéristiques du contenu"@fr,
        "anmärkning om förändringar i innehållsegenskaper"@sv ;
    reg:hasUnconstrained <http://rdaregistry.info/Elements/u/P60123> ;
    reg:lexicalAlias <http://rdaregistry.info/Elements/e/noteOnChangesInContentCharacteristics.en> ;
    reg:name "noteOnChangesInContentCharacteristics"@en ;
    reg:status <http://metadataregistry.org/uri/RegStatus/1001> ;
    rdfs:domain <http://rdaregistry.info/Elements/c/C10006> ;
    rdfs:isDefinedBy <http://rdaregistry.info/Elements/e/> ;
    rdfs:subPropertyOf <http://rdaregistry.info/Elements/e/P20071> ;
    skos:definition "Relates an expression to a note on changes in content characteristics that occur in subsequent issues or parts of an expression issued in successive parts or between iterations of an integrating resource."@en .

<http://rdaregistry.info/Elements/e/P20014> a rdf:Property ;
    rdfs:label "has dancer"@en ;
    rdakit:instructionNumber "18.5" ;
    rdakit:toolkitDefinition "A performer contributing to an expression of a work by dancing in a musical, dramatic, etc., presentation."@en,
        "Un intérprete que contribuye a una expresión de una obra danzando en una presentación musical, dramática, etc."@es,
        "Interprète contribuant à une expression d’une œuvre en dansant dans une représentation musicale ou dramatique, etc."@fr ;
    rdakit:toolkitLabel "dancer"@en,
        "bailarín"@es,
        "danseur"@fr ;
    reg:hasSubproperty <http://rdaregistry.info/Elements/e/object/P20014> ;
    reg:hasUnconstrained <http://rdaregistry.info/Elements/u/P60144> ;
    reg:lexicalAlias <http://rdaregistry.info/Elements/e/dancer.en> ;
    reg:name "dancer"@en ;
    reg:status <http://metadataregistry.org/uri/RegStatus/1001> ;
    rdfs:domain <http://rdaregistry.info/Elements/c/C10006> ;
    rdfs:isDefinedBy <http://rdaregistry.info/Elements/e/> ;
    rdfs:subPropertyOf <http://rdaregistry.info/Elements/e/P20039> ;
    skos:definition "Relates an expression to a performer contributing to an expression of a work by dancing in a musical, dramatic, etc., presentation."@en .

<http://rdaregistry.info/Elements/e/P20015> a rdf:Property ;
    rdfs:label "has instructor"@en ;
    rdakit:instructionNumber "18.5" ;
    rdakit:toolkitDefinition "A performer contributing to an expression of a work by teaching or providing a demonstration."@en,
        "Un intérprete que contribuye a una expresión de una obra impartiendo formación o proporcionando una demostración."@es,
        "Interprète contribuant à une expression d’une œuvre en transmettant des connaissances par la théorie ou la pratique."@fr ;
    rdakit:toolkitLabel "instructor"@en,
        "profesor"@es,
        "enseignant"@fr ;
    reg:hasSubproperty <http://rdaregistry.info/Elements/e/object/P20015> ;
    reg:hasUnconstrained <http://rdaregistry.info/Elements/u/P60145> ;
    reg:lexicalAlias <http://rdaregistry.info/Elements/e/instructor.en> ;
    reg:name "instructor"@en ;
    reg:status <http://metadataregistry.org/uri/RegStatus/1001> ;
    rdfs:domain <http://rdaregistry.info/Elements/c/C10006> ;
    rdfs:isDefinedBy <http://rdaregistry.info/Elements/e/> ;
    rdfs:subPropertyOf <http://rdaregistry.info/Elements/e/P20039> ;
    skos:definition "Relates an expression to a performer contributing to an expression of a work by teaching or providing a demonstration."@en .

<http://rdaregistry.info/Elements/e/P20016> a rdf:Property ;
    rdfs:label "has host"@en ;
    rdakit:instructionNumber "18.5" ;
    rdakit:toolkitDefinition "A performer contributing to an expression of a work by leading a program, often broadcast, that includes other guests, performers, etc."@en,
        "Un intérprete que contribuye a una expresión de una obra dirigiendo un programa (a menudo una transmisión) que incluye otros invitados, intérpretes, etc., ( por ej., presentadores de programas de debates)."@es,
        "Interprète contribuant à une expression d’une œuvre en dirigeant une émission (souvent diffusée) qui comprend d’autres invités, interprètes, etc. (par exemple, un animateur d’émission-débat)."@fr ;
    rdakit:toolkitLabel "host"@en,
        "presentador"@es,
        "hôte"@fr ;
    reg:hasSubproperty <http://rdaregistry.info/Elements/e/object/P20016> ;
    reg:hasUnconstrained <http://rdaregistry.info/Elements/u/P60146> ;
    reg:lexicalAlias <http://rdaregistry.info/Elements/e/host.en> ;
    reg:name "host"@en ;
    reg:status <http://metadataregistry.org/uri/RegStatus/1001> ;
    rdfs:domain <http://rdaregistry.info/Elements/c/C10006> ;
    rdfs:isDefinedBy <http://rdaregistry.info/Elements/e/> ;
    rdfs:subPropertyOf <http://rdaregistry.info/Elements/e/P20039> ;
    skos:definition "Relates an expression to a performer contributing to an expression of a work by leading a program, often broadcast, that includes other guests, performers, etc."@en .

<http://rdaregistry.info/Elements/e/P20017> a rdf:Property ;
    rdfs:label "has moderator"@en ;
    rdakit:instructionNumber "18.5" ;
    rdakit:toolkitDefinition "A performer contributing to an expression of a work by leading a program, often broadcast, where topics are discussed, usually with participation of experts in fields related to the discussion."@en,
        "Un intérprete que contribuye a una expresión de una obra dirigiendo un programa (a menudo una transmisión) en el cual los temas se discuten generalmente con la participación de expertos en esos temas."@es,
        "Interprète contribuant à une expression d’une œuvre en dirigeant une émission (souvent diffusée) où des sujets sont discutés, habituellement avec la participation d’experts dans les domaines reliés à la discussion."@fr ;
    rdakit:toolkitLabel "moderator"@en,
        "moderador"@es,
        "modérateur"@fr ;
    reg:hasSubproperty <http://rdaregistry.info/Elements/e/object/P20017> ;
    reg:hasUnconstrained <http://rdaregistry.info/Elements/u/P60147> ;
    reg:lexicalAlias <http://rdaregistry.info/Elements/e/moderator.en> ;
    reg:name "moderator"@en ;
    reg:status <http://metadataregistry.org/uri/RegStatus/1001> ;
    rdfs:domain <http://rdaregistry.info/Elements/c/C10006> ;
    rdfs:isDefinedBy <http://rdaregistry.info/Elements/e/> ;
    rdfs:subPropertyOf <http://rdaregistry.info/Elements/e/P20039> ;
    skos:definition "Relates an expression to a performer contributing to an expression of a work by leading a program, often broadcast, where topics are discussed, usually with participation of experts in fields related to the discussion."@en .

<http://rdaregistry.info/Elements/e/P20018> a rdf:Property ;
    rdfs:label "has puppeteer"@en ;
    rdakit:instructionNumber "18.5" ;
    rdakit:toolkitDefinition "A performer contributing to an expression of a work by manipulating, controlling, or directing puppets or marionettes in a moving image production or a musical or dramatic presentation or entertainment."@en,
        "Un intérprete que contribuye a una expresión de una obra manipulando, controlando o dirigiendo títeres o marionetas en una producción de imágenes en movimiento o producción teatral, musical o un espectáculo."@es,
        "Interprète contribuant à une expression d’une œuvre en manipulant, en contrôlant ou en dirigeant des marionnettes dans une production d’images animées ou bien dans une représentation ou un spectacle musical ou dramatique."@fr ;
    rdakit:toolkitLabel "puppeteer"@en,
        "titiritero"@es,
        "marionnettiste"@fr ;
    reg:hasSubproperty <http://rdaregistry.info/Elements/e/object/P20018> ;
    reg:hasUnconstrained <http://rdaregistry.info/Elements/u/P60148> ;
    reg:lexicalAlias <http://rdaregistry.info/Elements/e/puppeteer.en> ;
    reg:name "puppeteer"@en ;
    reg:status <http://metadataregistry.org/uri/RegStatus/1001> ;
    rdfs:domain <http://rdaregistry.info/Elements/c/C10006> ;
    rdfs:isDefinedBy <http://rdaregistry.info/Elements/e/> ;
    rdfs:subPropertyOf <http://rdaregistry.info/Elements/e/P20039> ;
    skos:definition "Relates an expression to a performer contributing to an expression of a work by manipulating, controlling, or directing puppets or marionettes in a moving image production or a musical or dramatic presentation or entertainment."@en .

<http://rdaregistry.info/Elements/e/P20019> a rdf:Property ;
    rdfs:label "has panelist"@en ;
    rdakit:instructionNumber "18.5" ;
    rdakit:toolkitDefinition "A performer contributing to an expression of a work by participating in a program, often broadcast, where topics are discussed, usually with participation of experts in fields related to the discussion."@en,
        "Un intérprete que contribuye a una expresión de una obra participando en un programa (a menudo una transmisión) en el cual los temas se discuten generalmente con la participación de expertos en esos temas."@es,
        "Interprète contribuant à une expression d’une œuvre en participant à une émission (souvent diffusée) où des sujets sont discutés, habituellement avec la participation d’experts dans les domaines reliés à la discussion."@fr ;
    rdakit:toolkitLabel "panelist"@en,
        "panelista"@es,
        "panéliste"@fr ;
    reg:hasSubproperty <http://rdaregistry.info/Elements/e/object/P20019> ;
    reg:hasUnconstrained <http://rdaregistry.info/Elements/u/P60149> ;
    reg:lexicalAlias <http://rdaregistry.info/Elements/e/panelist.en> ;
    reg:name "panelist"@en ;
    reg:status <http://metadataregistry.org/uri/RegStatus/1001> ;
    rdfs:domain <http://rdaregistry.info/Elements/c/C10006> ;
    rdfs:isDefinedBy <http://rdaregistry.info/Elements/e/> ;
    rdfs:subPropertyOf <http://rdaregistry.info/Elements/e/P20039> ;
    skos:definition "Relates an expression to a performer contributing to an expression of a work by participating in a program, often broadcast, where topics are discussed, usually with participation of experts in fields related to the discussion."@en .

<http://rdaregistry.info/Elements/e/P20020> a rdf:Property ;
    rdfs:label "has instrumentalist"@en ;
    rdakit:instructionNumber "18.5" ;
    rdakit:toolkitDefinition "A performer contributing to an expression of a work by playing a musical instrument."@en,
        "Un intérprete que contribuye a una expresión de una obra tocando un instrumento musical."@es,
        "Interprète contribuant à une expression d’une œuvre en jouant d’un instrument de musique."@fr ;
    rdakit:toolkitLabel "instrumentalist"@en,
        "instrumentista"@es,
        "instrumentiste"@fr ;
    reg:hasSubproperty <http://rdaregistry.info/Elements/e/object/P20020> ;
    reg:hasUnconstrained <http://rdaregistry.info/Elements/u/P60150> ;
    reg:lexicalAlias <http://rdaregistry.info/Elements/e/instrumentalist.en> ;
    reg:name "instrumentalist"@en ;
    reg:status <http://metadataregistry.org/uri/RegStatus/1001> ;
    rdfs:domain <http://rdaregistry.info/Elements/c/C10006> ;
    rdfs:isDefinedBy <http://rdaregistry.info/Elements/e/> ;
    rdfs:subPropertyOf <http://rdaregistry.info/Elements/e/P20039> ;
    skos:definition "Relates an expression to a performer contributing to an expression of a work by playing a musical instrument."@en .

<http://rdaregistry.info/Elements/e/P20021> a rdf:Property ;
    rdfs:label "has commentator"@en ;
    rdakit:instructionNumber "18.5" ;
    rdakit:toolkitDefinition "A performer contributing to an expression of a work by providing interpretation, analysis, or a discussion of the subject matter on a recording, film, or other audiovisual medium."@en,
        "Un intérprete que contribuye a una expresión de una obra dando una interpretación, análisis, o una discusión del tema en una grabación, película u otro medio audiovisual."@es,
        "Interprète contribuant à une expression d’une œuvre en fournissant une interprétation, une analyse ou une explication du sujet sur un enregistrement, un film ou un autre support audiovisuel."@fr ;
    rdakit:toolkitLabel "commentator"@en,
        "comentarista"@es,
        "commentateur"@fr ;
    reg:hasSubproperty <http://rdaregistry.info/Elements/e/object/P20021> ;
    reg:hasUnconstrained <http://rdaregistry.info/Elements/u/P60151> ;
    reg:lexicalAlias <http://rdaregistry.info/Elements/e/commentator.en> ;
    reg:name "commentator"@en ;
    reg:status <http://metadataregistry.org/uri/RegStatus/1001> ;
    rdfs:domain <http://rdaregistry.info/Elements/c/C10006> ;
    rdfs:isDefinedBy <http://rdaregistry.info/Elements/e/> ;
    rdfs:subPropertyOf <http://rdaregistry.info/Elements/e/P20039> ;
    skos:definition "Relates an expression to a performer contributing to an expression of a work by providing interpretation, analysis, or a discussion of the subject matter on a recording, film, or other audiovisual medium."@en .

<http://rdaregistry.info/Elements/e/P20022> a rdf:Property ;
    rdfs:label "has narrator"@en ;
    rdakit:instructionNumber "18.5" ;
    rdakit:toolkitDefinition "A performer contributing to an expression of a work by reading aloud or giving an account of an act, occurrence, course of events, etc."@en,
        "Un intérprete que contribuye a una expresión de una obra leyendo en voz alta o hablando para dar cuenta de un acto, acontecimiento, desarrollo de eventos, etc."@es,
        "Interprète contribuant à une expression d’une œuvre en lisant à voix haute ou en rendant compte d’une action, d’une situation, du déroulement des événements, etc."@fr ;
    rdakit:toolkitLabel "narrator"@en,
        "narrador"@es,
        "narrateur"@fr ;
    reg:hasSubproperty <http://rdaregistry.info/Elements/e/object/P20022> ;
    reg:hasUnconstrained <http://rdaregistry.info/Elements/u/P60153> ;
    reg:lexicalAlias <http://rdaregistry.info/Elements/e/narrator.en> ;
    reg:name "narrator"@en ;
    reg:status <http://metadataregistry.org/uri/RegStatus/1001> ;
    rdfs:domain <http://rdaregistry.info/Elements/c/C10006> ;
    rdfs:isDefinedBy <http://rdaregistry.info/Elements/e/> ;
    rdfs:subPropertyOf <http://rdaregistry.info/Elements/e/P20039> ;
    skos:definition "Relates an expression to a performer contributing to an expression of a work by reading aloud or giving an account of an act, occurrence, course of events, etc."@en .

<http://rdaregistry.info/Elements/e/P20023> a rdf:Property ;
    rdfs:label "has storyteller"@en ;
    rdakit:instructionNumber "18.5" ;
    rdakit:toolkitDefinition "A performer contributing to an expression of a work by relaying a creator's original story with dramatic or theatrical interpretation."@en,
        "Un intérprete que contribuye a una expresión de una obra contando una historia de un creador original mediante una interpretación dramática o teatral."@es,
        "Interprète contribuant à une expression d’une œuvre en racontant l’histoire originale d’un créateur dans une interprétation dramatique ou théâtrale."@fr ;
    rdakit:toolkitLabel "storyteller"@en,
        "narrador de cuentos"@es,
        "conteur"@fr ;
    reg:hasSubproperty <http://rdaregistry.info/Elements/e/object/P20023> ;
    reg:hasUnconstrained <http://rdaregistry.info/Elements/u/P60154> ;
    reg:lexicalAlias <http://rdaregistry.info/Elements/e/storyteller.en> ;
    reg:name "storyteller"@en ;
    reg:status <http://metadataregistry.org/uri/RegStatus/1001> ;
    rdfs:domain <http://rdaregistry.info/Elements/c/C10006> ;
    rdfs:isDefinedBy <http://rdaregistry.info/Elements/e/> ;
    rdfs:subPropertyOf <http://rdaregistry.info/Elements/e/P20039> ;
    skos:definition "Relates an expression to a performer contributing to an expression of a work by relaying a creator's original story with dramatic or theatrical interpretation."@en .

<http://rdaregistry.info/Elements/e/P20024> a rdf:Property ;
    rdfs:label "has speaker"@en ;
    rdakit:instructionNumber "18.5" ;
    rdakit:toolkitDefinition "A performer contributing to an expression of a work by speaking words, such as a lecture, speech, etc."@en,
        "Un intérprete que contribuye a una expresión de una obra haciendo u ofreciendo conferencias, discursos, etc."@es,
        "Interprète contribuant à une expression d’une œuvre en énonçant des paroles, telles qu’un exposé, un discours, etc."@fr ;
    rdakit:toolkitLabel "speaker"@en,
        "conferenciante"@es,
        "orateur"@fr ;
    reg:hasSubproperty <http://rdaregistry.info/Elements/e/object/P20024> ;
    reg:hasUnconstrained <http://rdaregistry.info/Elements/u/P60155> ;
    reg:lexicalAlias <http://rdaregistry.info/Elements/e/speaker.en> ;
    reg:name "speaker"@en ;
    reg:status <http://metadataregistry.org/uri/RegStatus/1001> ;
    rdfs:domain <http://rdaregistry.info/Elements/c/C10006> ;
    rdfs:isDefinedBy <http://rdaregistry.info/Elements/e/> ;
    rdfs:subPropertyOf <http://rdaregistry.info/Elements/e/P20039> ;
    skos:definition "Relates an expression to a performer contributing to an expression of a work by speaking words, such as a lecture, speech, etc."@en .

<http://rdaregistry.info/Elements/e/P20025> a rdf:Property ;
    rdfs:label "has singer"@en ;
    rdakit:instructionNumber "18.5" ;
    rdakit:toolkitDefinition "A performer contributing to an expression of a work by using his/her/their voice, with or without instrumental accompaniment, to produce music."@en,
        "Un intérprete que contribuye a una expresión de una obra usando su voz, sus voces, con o sin acompañamiento instrumental, para producir música."@es,
        "Interprète contribuant à une expression d’une œuvre en utilisant sa voix, avec ou sans accompagnement instrumental, pour produire de la musique."@fr ;
    rdakit:toolkitLabel "singer"@en,
        "cantante"@es,
        "chanteur"@fr ;
    reg:hasSubproperty <http://rdaregistry.info/Elements/e/object/P20025> ;
    reg:hasUnconstrained <http://rdaregistry.info/Elements/u/P60156> ;
    reg:lexicalAlias <http://rdaregistry.info/Elements/e/singer.en> ;
    reg:name "singer"@en ;
    reg:status <http://metadataregistry.org/uri/RegStatus/1001> ;
    rdfs:domain <http://rdaregistry.info/Elements/c/C10006> ;
    rdfs:isDefinedBy <http://rdaregistry.info/Elements/e/> ;
    rdfs:subPropertyOf <http://rdaregistry.info/Elements/e/P20039> ;
    skos:definition "Relates an expression to a performer contributing to an expression of a work by using his/her/their voice, with or without instrumental accompaniment, to produce music."@en ;
    skos:scopeNote "A singer's performance may or may not include actual words."@en .

<http://rdaregistry.info/Elements/e/P20026> a rdf:Property ;
    rdfs:label "has composer (expression)"@en ;
    rdakit:instructionNumber "18.5" ;
    rdakit:toolkitDefinition "An agent contributing to an expression by adding music to a work that originally lacked it, by composing new music to substitute for original music, or by composing new music to supplement existing music."@en,
        "Una persona, familia o entidad corporativa que contribuye a una expresión agregando música a una obra que originalmente no tenía, componiendo música nueva para sustituir la música original, o componiendo nueva música para complementar la música existente."@es,
        "Personne, famille ou collectivité contribuant à une expression en ajoutant de la musique à une œuvre qui n’en avait pas à l’origine, en composant une nouvelle musique pour remplacer la musique originale ou en composant une nouvelle musique pour compléter la musique existante."@fr ;
    rdakit:toolkitLabel "composer (expression)"@en,
        "compositor (expresión)"@es,
        "compositeur (expression)"@fr ;
    reg:hasSubproperty <http://rdaregistry.info/Elements/e/object/P20026> ;
    reg:hasUnconstrained <http://rdaregistry.info/Elements/u/P60426> ;
    reg:lexicalAlias <http://rdaregistry.info/Elements/e/composerExpression.en> ;
    reg:name "composerExpression"@en ;
    reg:status <http://metadataregistry.org/uri/RegStatus/1001> ;
    rdfs:domain <http://rdaregistry.info/Elements/c/C10006> ;
    rdfs:isDefinedBy <http://rdaregistry.info/Elements/e/> ;
    rdfs:subPropertyOf <http://rdaregistry.info/Elements/e/P20053> ;
    skos:definition "Relates an expression to an agent contributing to an expression by adding music to a work that originally lacked it, by composing new music to substitute for original music, or by composing new music to supplement existing music."@en .

<http://rdaregistry.info/Elements/e/P20027> a rdf:Property ;
    rdfs:label "has surveyor"@en ;
    rdakit:instructionNumber "18.5" ;
    rdakit:toolkitDefinition "An agent contributing to an expression of a cartographic work by providing measurements or dimensional relationships for a geographic area represented."@en,
        "Una persona, familia o entidad corporativa que contribuye a una expresión de una obra cartográfica proporcionando medidas o relaciones dimensionales para el área geográfica representada."@es,
        "Personne, famille ou collectivité contribuant à une expression d’une œuvre cartographique en fournissant les mesures ou les relations dimensionnelles pour  l’aire géographique représentée."@fr ;
    rdakit:toolkitLabel "surveyor"@en,
        "topógrafo"@es,
        "arpenteur"@fr ;
    reg:hasSubproperty <http://rdaregistry.info/Elements/e/object/P20027> ;
    reg:hasUnconstrained <http://rdaregistry.info/Elements/u/P60377> ;
    reg:lexicalAlias <http://rdaregistry.info/Elements/e/surveyor.en> ;
    reg:name "surveyor"@en ;
    reg:status <http://metadataregistry.org/uri/RegStatus/1001> ;
    rdfs:domain <http://rdaregistry.info/Elements/c/C10006> ;
    rdfs:isDefinedBy <http://rdaregistry.info/Elements/e/> ;
    rdfs:subPropertyOf <http://rdaregistry.info/Elements/e/P20053> ;
    skos:definition "Relates an expression to an agent contributing to an expression of a cartographic work by providing measurements or dimensional relationships for a geographic area represented."@en .

<http://rdaregistry.info/Elements/e/P20028> a rdf:Property ;
    rdfs:label "has animator"@en ;
    rdakit:instructionNumber "18.5" ;
    rdakit:seeAlso <http://rdaregistry.info/Elements/w/P10058> ;
    rdakit:toolkitDefinition "An agent contributing to an expression of a moving image work or computer program by giving apparent movement to inanimate objects or drawings."@en,
        "Una persona, familia o entidad corporativa que contribuye a una expresión de una obra de imagen en movimiento o un programa de computadora dando movimiento aparente a objetos o dibujos inanimados."@es,
        "Personne, famille ou collectivité contribuant à une expression d’une œuvre d’images animées ou d’un programme informatique en donnant l’illusion du mouvement à des objets inanimés ou à des dessins."@fr ;
    rdakit:toolkitLabel "animator"@en,
        "animador"@es,
        "animateur"@fr ;
    reg:hasSubproperty <http://rdaregistry.info/Elements/e/object/P20028> ;
    reg:hasUnconstrained <http://rdaregistry.info/Elements/u/P60378> ;
    reg:lexicalAlias <http://rdaregistry.info/Elements/e/animator.en> ;
    reg:name "animator"@en ;
    reg:status <http://metadataregistry.org/uri/RegStatus/1001> ;
    rdfs:domain <http://rdaregistry.info/Elements/c/C10006> ;
    rdfs:isDefinedBy <http://rdaregistry.info/Elements/e/> ;
    rdfs:subPropertyOf <http://rdaregistry.info/Elements/e/P20053> ;
    skos:definition "Relates an expression to an agent contributing to an expression of a moving image work or computer program by giving apparent movement to inanimate objects or drawings."@en ;
    skos:scopeNote "Creation of the drawings that are animated is excluded."@en .

<http://rdaregistry.info/Elements/e/P20031> a rdf:Property ;
    rdfs:label "has stage director"@en ;
    rdakit:instructionNumber "18.5" ;
    rdakit:toolkitDefinition "An agent contributing to an expression of a stage work through the general management and supervision of a performance."@en,
        "Una persona, familia o entidad corporativa que contribuye a una expresión de una obra escénica mediante la dirección y supervisión general de una interpretación."@es,
        "Personne, famille ou collectivité contribuant à une expression d’une œuvre scénique par la gestion et la supervision générales d’une prestation."@fr ;
    rdakit:toolkitLabel "stage director"@en,
        "director de escena"@es,
        "metteur en scène"@fr ;
    reg:hasSubproperty <http://rdaregistry.info/Elements/e/object/P20031> ;
    reg:hasUnconstrained <http://rdaregistry.info/Elements/u/P60399> ;
    reg:lexicalAlias <http://rdaregistry.info/Elements/e/stageDirector.en> ;
    reg:name "stageDirector"@en ;
    reg:status <http://metadataregistry.org/uri/RegStatus/1001> ;
    rdfs:domain <http://rdaregistry.info/Elements/c/C10006> ;
    rdfs:isDefinedBy <http://rdaregistry.info/Elements/e/> ;
    rdfs:subPropertyOf <http://rdaregistry.info/Elements/e/P20053> ;
    skos:definition "Relates an expression to an agent contributing to an expression of a stage work through the general management and supervision of a performance."@en .

<http://rdaregistry.info/Elements/e/P20032> a rdf:Property ;
    rdfs:label "has interviewer (expression)"@en ;
    rdakit:instructionNumber "18.5" ;
    rdakit:toolkitDefinition "An agent contributing to an expression of a work by acting as an interviewer, reporter, pollster, or some other information gathering agent."@en,
        "Una persona, familia o entidad corporativa que contribuye a una expresión de una obra actuando como entrevistador, reportero, encuestador, o algún otro agente recolector de información."@es,
        "Personne, famille ou collectivité contribuant à une expression d’une œuvre en agissant à titre d’intervieweur, de journaliste, de sondeur ou d’autre agent recueillant de l’information."@fr ;
    rdakit:toolkitLabel "interviewer (expression)"@en,
        "entrevistador (expresión)"@es,
        "intervieweur (expression)"@fr ;
    reg:hasSubproperty <http://rdaregistry.info/Elements/e/object/P20032> ;
    reg:hasUnconstrained <http://rdaregistry.info/Elements/u/P60430> ;
    reg:lexicalAlias <http://rdaregistry.info/Elements/e/interviewerExpression.en> ;
    reg:name "interviewerExpression"@en ;
    reg:status <http://metadataregistry.org/uri/RegStatus/1001> ;
    rdfs:domain <http://rdaregistry.info/Elements/c/C10006> ;
    rdfs:isDefinedBy <http://rdaregistry.info/Elements/e/> ;
    rdfs:subPropertyOf <http://rdaregistry.info/Elements/e/P20053> ;
    skos:definition "Relates an expression to an agent contributing to an expression of a work by acting as an interviewer, reporter, pollster, or some other information gathering agent."@en .

<http://rdaregistry.info/Elements/e/P20033> a rdf:Property ;
    rdfs:label "has draftsman"@en ;
    rdakit:instructionNumber "18.5" ;
    rdakit:toolkitDefinition "An agent contributing to an expression of a work by an architect, inventor, etc., by making detailed plans or drawings for buildings, ships, aircraft, machines, objects, etc."@en,
        "Una persona, familia o entidad corporativa que contribuye a una expresión de una obra de un arquitecto, inventor, etc., haciendo planos o dibujos detallados de edificios, barcos, aviones, máquinas, objetos, etc."@es,
        "Personne, famille ou collectivité contribuant à une expression d’une œuvre par un architecte, un inventeur, etc. en effectuant des plans ou des dessins détaillés pour des bâtiments, des navires, des avions, des machines, des objets, etc."@fr ;
    rdakit:toolkitLabel "draftsman"@en,
        "dibujante"@es,
        "dessinateur industriel"@fr ;
    reg:hasSubproperty <http://rdaregistry.info/Elements/e/object/P20033> ;
    reg:hasUnconstrained <http://rdaregistry.info/Elements/u/P60381> ;
    reg:lexicalAlias <http://rdaregistry.info/Elements/e/draftsman.en> ;
    reg:name "draftsman"@en ;
    reg:status <http://metadataregistry.org/uri/RegStatus/1001> ;
    rdfs:domain <http://rdaregistry.info/Elements/c/C10006> ;
    rdfs:isDefinedBy <http://rdaregistry.info/Elements/e/> ;
    rdfs:subPropertyOf <http://rdaregistry.info/Elements/e/P20053> ;
    skos:definition "Relates an expression to an agent contributing to an expression of a work by an architect, inventor, etc., by making detailed plans or drawings for buildings, ships, aircraft, machines, objects, etc."@en .

<http://rdaregistry.info/Elements/e/P20034> a rdf:Property ;
    rdfs:label "has transcriber"@en ;
    rdakit:instructionNumber "18.5" ;
    rdakit:seeAlso <http://rdaregistry.info/Elements/e/P20029> ;
    rdakit:toolkitDefinition "An agent contributing to an expression of a work by writing down or notating unwritten or unnotated content, or by changing it from one system of notation to another."@en,
        "Una persona, familia o entidad corporativa que contribuye a una expresión de una obra mediante la escritura o notación de contenido no escrito o no notado, o cambiando de un sistema de notación a otro."@es,
        "Personne, famille ou collectivité contribuant à une expression d’une œuvre en écrivant ou en notant un contenu auparavant non écrit ou non noté, ou bien en le transposant d’un système de notation à un autre."@fr ;
    rdakit:toolkitLabel "transcriber"@en,
        "transcriptor"@es,
        "transcripteur"@fr ;
    reg:hasSubproperty <http://rdaregistry.info/Elements/e/object/P20034> ;
    reg:hasUnconstrained <http://rdaregistry.info/Elements/u/P60382> ;
    reg:lexicalAlias <http://rdaregistry.info/Elements/e/transcriber.en> ;
    reg:name "transcriber"@en ;
    reg:status <http://metadataregistry.org/uri/RegStatus/1001> ;
    rdfs:domain <http://rdaregistry.info/Elements/c/C10006> ;
    rdfs:isDefinedBy <http://rdaregistry.info/Elements/e/> ;
    rdfs:subPropertyOf <http://rdaregistry.info/Elements/e/P20053> ;
    skos:definition "Relates an expression to an agent contributing to an expression of a work by writing down or notating unwritten or unnotated content, or by changing it from one system of notation to another."@en ;
    skos:scopeNote "Transcription of a musical work for a different instrument or performing group is excluded."@en .

<http://rdaregistry.info/Elements/e/P20035> a rdf:Property ;
    rdfs:label "has musical director"@en ;
    rdakit:instructionNumber "18.5" ;
    rdakit:toolkitDefinition "An agent contributing to an expression of a work by coordinating the activities of composers, sound editors, and sound mixers for a moving image production or for a musical or dramatic presentation or entertainment."@en,
        "Una persona, familia o entidad corporativa que contribuye a una expresión de una obra coordinando las actividades del compositor, el editor de sonido, y los mezcladores de sonido para una producción de una imagen en movimiento o para una producción teatral, musical o un espectáculo."@es,
        "Personne, famille ou collectivité contribuant à une expression d’une œuvre en coordonnant les activités du compositeur, du monteur son et des mixeurs de son pour une production d’images animées ou bien pour une représentation ou un spectacle dramatique ou musical."@fr ;
    rdakit:toolkitLabel "musical director"@en,
        "director musical"@es,
        "directeur musical"@fr ;
    reg:hasSubproperty <http://rdaregistry.info/Elements/e/object/P20035> ;
    reg:hasUnconstrained <http://rdaregistry.info/Elements/u/P60383> ;
    reg:lexicalAlias <http://rdaregistry.info/Elements/e/musicalDirector.en> ;
    reg:name "musicalDirector"@en ;
    reg:status <http://metadataregistry.org/uri/RegStatus/1001> ;
    rdfs:domain <http://rdaregistry.info/Elements/c/C10006> ;
    rdfs:isDefinedBy <http://rdaregistry.info/Elements/e/> ;
    rdfs:subPropertyOf <http://rdaregistry.info/Elements/e/P20053> ;
    skos:definition "Relates an expression to an agent contributing to an expression of a work by coordinating the activities of composers, sound editors, and sound mixers for a moving image production or for a musical or dramatic presentation or entertainment."@en .

<http://rdaregistry.info/Elements/e/P20036> a rdf:Property ;
    rdfs:label "has costume designer"@en ;
    rdakit:instructionNumber "18.5" ;
    rdakit:toolkitDefinition "An agent contributing to an expression of a work by designing costumes for a moving image production or for a musical or dramatic presentation or entertainment."@en,
        "Una persona, familia o entidad corporativa que contribuye a una expresión de una obra diseñando el vestuario para una producción de una imagen en movimiento o para una producción teatral o musical o un espectáculo."@es,
        "Personne, famille ou collectivité contribuant à une expression d’une œuvre en créant les costumes pour une production d’images animées ou bien pour une représentation ou un spectacle musical ou dramatique."@fr ;
    rdakit:toolkitLabel "costume designer"@en,
        "diseñador de vestuario"@es,
        "créateur de costumes"@fr ;
    reg:hasSubproperty <http://rdaregistry.info/Elements/e/object/P20036> ;
    reg:hasUnconstrained <http://rdaregistry.info/Elements/u/P60384> ;
    reg:lexicalAlias <http://rdaregistry.info/Elements/e/costumeDesigner.en> ;
    reg:name "costumeDesigner"@en ;
    reg:status <http://metadataregistry.org/uri/RegStatus/1001> ;
    rdfs:domain <http://rdaregistry.info/Elements/c/C10006> ;
    rdfs:isDefinedBy <http://rdaregistry.info/Elements/e/> ;
    rdfs:subPropertyOf <http://rdaregistry.info/Elements/e/P20053> ;
    skos:definition "Relates an expression to an agent contributing to an expression of a work by designing costumes for a moving image production or for a musical or dramatic presentation or entertainment."@en .

<http://rdaregistry.info/Elements/e/P20037> a rdf:Property ;
    rdfs:label "has translator"@en ;
    rdakit:instructionNumber "18.5" ;
    rdakit:toolkitDefinition "An agent contributing to an expression of a work by expressing the linguistic content of the work in a language different from that of previous expressions of the original work."@en,
        "Una persona, familia o entidad corporativa que contribuye a una expresión de una obra expresando el contenido linguístico de la obra en una lengua diferente de las expresiones previas de la obra."@es,
        "Personne, famille ou collectivité contribuant à une expression d’une œuvre en exprimant le texte original de l’œuvre dans une langue différente de celle de l’œuvre originale."@fr ;
    rdakit:toolkitLabel "translator"@en,
        "traductor"@es,
        "traducteur"@fr ;
    reg:hasSubproperty <http://rdaregistry.info/Elements/e/object/P20037> ;
    reg:hasUnconstrained <http://rdaregistry.info/Elements/u/P60385> ;
    reg:lexicalAlias <http://rdaregistry.info/Elements/e/translator.en> ;
    reg:name "translator"@en ;
    reg:status <http://metadataregistry.org/uri/RegStatus/1001> ;
    rdfs:domain <http://rdaregistry.info/Elements/c/C10006> ;
    rdfs:isDefinedBy <http://rdaregistry.info/Elements/e/> ;
    rdfs:subPropertyOf <http://rdaregistry.info/Elements/e/P20053> ;
    skos:definition "Relates an expression to an agent contributing to an expression of a work by expressing the linguistic content of the work in a language different from that of previous expressions of the original work."@en ;
    skos:scopeNote "Translation of linguistic content between forms of the same language from different time periods is included."@en .

<http://rdaregistry.info/Elements/e/P20038> a rdf:Property ;
    rdfs:label "has art director"@en ;
    rdakit:instructionNumber "18.5" ;
    rdakit:toolkitDefinition "An agent contributing to an expression of a work by overseeing artists and craftspeople who build sets for moving image productions."@en,
        "Una persona, familia o entidad corporativa que contribuye a una expresión de una obra supervisando los artistas y obreros que construyen los platos para producciones de imágenes en movimiento."@es,
        "Personne, famille ou collectivité contribuant à une expression d’une œuvre en supervisant les artistes et les artisans qui construisent les décors pour des productions d’images animées."@fr ;
    rdakit:toolkitLabel "art director"@en,
        "director artístico"@es,
        "directeur artistique"@fr ;
    reg:hasSubproperty <http://rdaregistry.info/Elements/e/object/P20038> ;
    reg:hasUnconstrained <http://rdaregistry.info/Elements/u/P60386> ;
    reg:lexicalAlias <http://rdaregistry.info/Elements/e/artDirector.en> ;
    reg:name "artDirector"@en ;
    reg:status <http://metadataregistry.org/uri/RegStatus/1001> ;
    rdfs:domain <http://rdaregistry.info/Elements/c/C10006> ;
    rdfs:isDefinedBy <http://rdaregistry.info/Elements/e/> ;
    rdfs:subPropertyOf <http://rdaregistry.info/Elements/e/P20053> ;
    skos:definition "Relates an expression to an agent contributing to an expression of a work by overseeing artists and craftspeople who build sets for moving image productions."@en .

<http://rdaregistry.info/Elements/e/P20040> a rdf:Property ;
    rdfs:label "has court reporter"@en ;
    rdakit:instructionNumber "18.5" ;
    rdakit:toolkitDefinition "An agent contributing to an expression of a work by preparing a court's opinions for publication."@en,
        "Una persona, familia o entidad corporativa que contribuye a una expresión de una obra preparando las opiniones del tribunal para publicación."@es,
        "Personne, famille ou collectivité contribuant à une expression d’une œuvre en préparant les opinions d’un tribunal aux fins de publication."@fr ;
    rdakit:toolkitLabel "court reporter"@en,
        "relator del tribunal"@es,
        "rapporteur judiciaire"@fr ;
    reg:hasSubproperty <http://rdaregistry.info/Elements/e/object/P20040> ;
    reg:hasUnconstrained <http://rdaregistry.info/Elements/u/P60388> ;
    reg:lexicalAlias <http://rdaregistry.info/Elements/e/courtReporter.en> ;
    reg:name "courtReporter"@en ;
    reg:status <http://metadataregistry.org/uri/RegStatus/1001> ;
    rdfs:domain <http://rdaregistry.info/Elements/c/C10006> ;
    rdfs:isDefinedBy <http://rdaregistry.info/Elements/e/> ;
    rdfs:subPropertyOf <http://rdaregistry.info/Elements/e/P20053> ;
    skos:definition "Relates an expression to an agent contributing to an expression of a work by preparing a court's opinions for publication."@en .

<http://rdaregistry.info/Elements/e/P20041> a rdf:Property ;
    rdfs:label "has writer of preface"@en ;
    rdakit:instructionNumber "18.5" ;
    rdakit:toolkitDefinition "An agent contributing to an expression of a work by providing a preface to an original work."@en,
        "Una persona, familia o entidad corporativa que contribuye a una expresión de una obra ofreciendo un prefacio a la obra original."@es,
        "Personne, famille ou collectivité contribuant à une expression d’une œuvre en fournissant une préface à l’œuvre originale."@fr ;
    rdakit:toolkitLabel "writer of preface"@en,
        "autor de prefacio"@es,
        "préfacier"@fr ;
    reg:hasSubproperty <http://rdaregistry.info/Elements/e/object/P20041> ;
    reg:hasUnconstrained <http://rdaregistry.info/Elements/u/P60389> ;
    reg:lexicalAlias <http://rdaregistry.info/Elements/e/writerOfPreface.en> ;
    reg:name "writerOfPreface"@en ;
    reg:status <http://metadataregistry.org/uri/RegStatus/1001> ;
    rdfs:domain <http://rdaregistry.info/Elements/c/C10006> ;
    rdfs:isDefinedBy <http://rdaregistry.info/Elements/e/> ;
    rdfs:subPropertyOf <http://rdaregistry.info/Elements/e/P20046> ;
    skos:definition "Relates an expression to an agent contributing to an expression of a work by providing a preface to an original work."@en .

<http://rdaregistry.info/Elements/e/P20042> a rdf:Property ;
    rdfs:label "has cartographer (expression)"@en ;
    rdakit:instructionNumber "18.5" ;
    rdakit:toolkitDefinition "An agent contributing to an expression of a work by providing additional cartography, or by modifying previous cartography."@en,
        "Una persona, familia o entidad corporativa que contribuye a una expresión de una obra proporcionando cartografía adicional o modificando la cartografía anterior."@es,
        "Personne, famille ou collectivité contribuant à une expression d’une œuvre en fournissant une cartographie additionnelle ou en modifiant la cartographie antérieure."@fr ;
    rdakit:toolkitLabel "cartographer (expression)"@en,
        "cartógrafo (expresión)"@es,
        "cartographe (expression)"@fr ;
    reg:hasSubproperty <http://rdaregistry.info/Elements/e/object/P20042> ;
    reg:hasUnconstrained <http://rdaregistry.info/Elements/u/P60425> ;
    reg:lexicalAlias <http://rdaregistry.info/Elements/e/cartographerExpression.en> ;
    reg:name "cartographerExpression"@en ;
    reg:status <http://metadataregistry.org/uri/RegStatus/1001> ;
    rdfs:domain <http://rdaregistry.info/Elements/c/C10006> ;
    rdfs:isDefinedBy <http://rdaregistry.info/Elements/e/> ;
    rdfs:subPropertyOf <http://rdaregistry.info/Elements/e/P20053> ;
    skos:definition "Relates an expression to an agent contributing to an expression of a work by providing additional cartography, or by modifying previous cartography."@en .

<http://rdaregistry.info/Elements/e/P20043> a rdf:Property ;
    rdfs:label "has choreographer (expression)"@en ;
    rdakit:instructionNumber "18.5" ;
    rdakit:toolkitDefinition "An agent contributing to an expression of a work by providing additional choreography, or by modifying previous choreography."@en,
        "Una persona, familia o entidad corporativa que contribuye a una expresión de una obra proporcionando coreografía adicional, o modificando la coreografía anterior."@es,
        "Personne, famille ou collectivité contribuant à une expression d’une œuvre en fournissant une chorégraphie additionnelle ou en modifiant la chorégraphie antérieure."@fr ;
    rdakit:toolkitLabel "choreographer (expression)"@en,
        "coreógrafo (expresión)"@es,
        "chorégraphe (expression)"@fr ;
    reg:hasSubproperty <http://rdaregistry.info/Elements/e/object/P20043> ;
    reg:hasUnconstrained <http://rdaregistry.info/Elements/u/P60433> ;
    reg:lexicalAlias <http://rdaregistry.info/Elements/e/choreographerExpression.en> ;
    reg:name "choreographerExpression"@en ;
    reg:status <http://metadataregistry.org/uri/RegStatus/1001> ;
    rdfs:domain <http://rdaregistry.info/Elements/c/C10006> ;
    rdfs:isDefinedBy <http://rdaregistry.info/Elements/e/> ;
    rdfs:subPropertyOf <http://rdaregistry.info/Elements/e/P20053> ;
    skos:definition "Relates an expression to an agent contributing to an expression of a work by providing additional choreography, or by modifying previous choreography."@en .

<http://rdaregistry.info/Elements/e/P20044> a rdf:Property ;
    rdfs:label "has writer of added commentary"@en ;
    rdakit:instructionNumber "18.5" ;
    rdakit:toolkitDefinition "An agent contributing to an expression of a work by providing an interpretation or critical explanation of an original work."@en,
        "Una persona, familia o entidad corporativa que contribuye a una expresión de una obra ofreciendo una interpretación o explicación crítica de la obra original."@es,
        "Personne, famille ou collectivité contribuant à une expression d’une œuvre en fournissant une interprétation ou une critique de l’œuvre originale."@fr ;
    rdakit:toolkitLabel "writer of added commentary"@en,
        "autor de comentario adicional"@es,
        "auteur de commentaire ajouté"@fr ;
    reg:hasSubproperty <http://rdaregistry.info/Elements/e/object/P20044> ;
    reg:hasUnconstrained <http://rdaregistry.info/Elements/u/P60390> ;
    reg:lexicalAlias <http://rdaregistry.info/Elements/e/writerOfAddedCommentary.en> ;
    reg:name "writerOfAddedCommentary"@en ;
    reg:status <http://metadataregistry.org/uri/RegStatus/1001> ;
    rdfs:domain <http://rdaregistry.info/Elements/c/C10006> ;
    rdfs:isDefinedBy <http://rdaregistry.info/Elements/e/> ;
    rdfs:subPropertyOf <http://rdaregistry.info/Elements/e/P20046> ;
    skos:definition "Relates an expression to an agent contributing to an expression of a work by providing an interpretation or critical explanation of an original work."@en .

<http://rdaregistry.info/Elements/e/P20045> a rdf:Property ;
    rdfs:label "has writer of introduction"@en ;
    rdakit:instructionNumber "18.5" ;
    rdakit:toolkitDefinition "An agent contributing to an expression of a work by providing an introduction to an original work."@en,
        "Una persona, familia o entidad corporativa que contribuye a una expresión de una obra ofreciendo una introducción a la obra original."@es,
        "Personne, famille ou collectivité contribuant à une expression d’une œuvre en fournissant une introduction à l’œuvre originale."@fr ;
    rdakit:toolkitLabel "writer of introduction"@en,
        "autor de introducción"@es,
        "auteur d’introduction"@fr ;
    reg:hasSubproperty <http://rdaregistry.info/Elements/e/object/P20045> ;
    reg:hasUnconstrained <http://rdaregistry.info/Elements/u/P60391> ;
    reg:lexicalAlias <http://rdaregistry.info/Elements/e/writerOfIntroduction.en> ;
    reg:name "writerOfIntroduction"@en ;
    reg:status <http://metadataregistry.org/uri/RegStatus/1001> ;
    rdfs:domain <http://rdaregistry.info/Elements/c/C10006> ;
    rdfs:isDefinedBy <http://rdaregistry.info/Elements/e/> ;
    rdfs:subPropertyOf <http://rdaregistry.info/Elements/e/P20046> ;
    skos:definition "Relates an expression to an agent contributing to an expression of a work by providing an introduction to an original work."@en .

<http://rdaregistry.info/Elements/e/P20047> a rdf:Property ;
    rdfs:label "has interviewee (expression)"@en ;
    rdakit:instructionNumber "18.5" ;
    rdakit:toolkitDefinition "An agent contributing to an expression of a work by responding to an interviewer, usually a reporter, pollster, or some other information gathering agent."@en,
        "Una persona, familia o entidad corporativa que contribuye a una expresión de una obra respondiendo a un entrevistador, generalmente un reportero, encuestador, o algún otro agente recolector de información."@es,
        "Personne, famille ou collectivité contribuant à une expression d’une œuvre en répondant à un intervieweur, habituellement un journaliste, un sondeur ou un autre agent recueillant de l’information."@fr ;
    rdakit:toolkitLabel "interviewee (expression)"@en,
        "entrevistado (expresión)"@es,
        "interviewé (expression)"@fr ;
    reg:hasSubproperty <http://rdaregistry.info/Elements/e/object/P20047> ;
    reg:hasUnconstrained <http://rdaregistry.info/Elements/u/P60432> ;
    reg:lexicalAlias <http://rdaregistry.info/Elements/e/intervieweeExpression.en> ;
    reg:name "intervieweeExpression"@en ;
    reg:status <http://metadataregistry.org/uri/RegStatus/1001> ;
    rdfs:domain <http://rdaregistry.info/Elements/c/C10006> ;
    rdfs:isDefinedBy <http://rdaregistry.info/Elements/e/> ;
    rdfs:subPropertyOf <http://rdaregistry.info/Elements/e/P20053> ;
    skos:definition "Relates an expression to an agent contributing to an expression of a work by responding to an interviewer, usually a reporter, pollster, or some other information gathering agent."@en .

<http://rdaregistry.info/Elements/e/P20048> a rdf:Property ;
    rdfs:label "has editor"@en ;
    rdakit:instructionNumber "18.5" ;
    rdakit:seeAlso <http://rdaregistry.info/Elements/w/P10061> ;
    rdakit:toolkitDefinition "An agent contributing to an expression of a work by revising or clarifying the content, or by selecting and putting together works, or parts of works, by one or more creators."@en,
        "Una persona, familia o entidad corporativa que contribuye a una expresión de una obra revisando o aclarando el contenido, por ej., agregando una introducción, notas u otro material crítico."@es,
        "Personne, famille ou collectivité contribuant à une expression d’une œuvre en révisant ou en clarifiant le contenu, ou bien en choisissant et en rassemblant des œuvres, ou des parties d’œuvres, d’un ou de plusieurs créateurs."@fr ;
    rdakit:toolkitLabel "editor"@en,
        "editor"@es,
        "éditeur intellectuel"@fr ;
    reg:hasSubproperty <http://rdaregistry.info/Elements/e/object/P20048> ;
    reg:hasUnconstrained <http://rdaregistry.info/Elements/u/P60393> ;
    reg:lexicalAlias <http://rdaregistry.info/Elements/e/editor.en> ;
    reg:name "editor"@en ;
    reg:status <http://metadataregistry.org/uri/RegStatus/1001> ;
    rdfs:domain <http://rdaregistry.info/Elements/c/C10006> ;
    rdfs:isDefinedBy <http://rdaregistry.info/Elements/e/> ;
    rdfs:subPropertyOf <http://rdaregistry.info/Elements/e/P20053> ;
    skos:definition "Relates an expression to an agent contributing to an expression of a work by revising or clarifying the content, or by selecting and putting together works, or parts of works, by one or more creators."@en ;
    skos:scopeNote "Addition of an introduction, notes, or other critical matter, or preparing an expression of a work for production, publication, or distribution is included. Major revision, adaptation, etc., that substantially changes the nature and content of the original work, resulting in a new work, is excluded."@en .

<http://rdaregistry.info/Elements/e/P20049> a rdf:Property ;
    rdfs:label "has abridger"@en ;
    rdakit:instructionNumber "18.5" ;
    rdakit:seeAlso <http://rdaregistry.info/Elements/w/P10061> ;
    rdakit:toolkitDefinition "An agent contributing to an expression of a work by shortening or condensing an original work but leaving the nature and content substantially unchanged."@en,
        "Una persona, familia o entidad corporativa que contribuye a una expresión de una obra acortando o condensando la obra original pero dejando intacta la naturaleza y el contenido de la obra original."@es,
        "Personne, famille ou collectivité contribuant à une expression d’une œuvre en abrégeant ou en condensant l’œuvre originale tout en conservant la nature et le contenu de l’œuvre originale sensiblement inchangés."@fr ;
    rdakit:toolkitLabel "abridger"@en,
        "responsable de la edición abreviada/abreviador"@es,
        "abréviateur"@fr ;
    reg:hasSubproperty <http://rdaregistry.info/Elements/e/object/P20049> ;
    reg:hasUnconstrained <http://rdaregistry.info/Elements/u/P60394> ;
    reg:lexicalAlias <http://rdaregistry.info/Elements/e/abridger.en> ;
    reg:name "abridger"@en ;
    reg:status <http://metadataregistry.org/uri/RegStatus/1001> ;
    rdfs:domain <http://rdaregistry.info/Elements/c/C10006> ;
    rdfs:isDefinedBy <http://rdaregistry.info/Elements/e/> ;
    rdfs:subPropertyOf <http://rdaregistry.info/Elements/e/P20053> ;
    skos:definition "Relates an expression to an agent contributing to an expression of a work by shortening or condensing an original work but leaving the nature and content substantially unchanged."@en ;
    skos:scopeNote "Substantial modification that results in the creation of a new work is excluded."@en .

<http://rdaregistry.info/Elements/e/P20050> a rdf:Property ;
    rdfs:label "has recording engineer"@en ;
    rdakit:instructionNumber "18.5" ;
    rdakit:toolkitDefinition "An audio engineer contributing to the audio content of an expression by supervising the technical aspects of a recording session."@en,
        "Una persona, familia o entidad corporativa que contribuye a una expresión de una obra supervisando los aspectos técnicos de una sesión de grabación de sonido o video."@es,
        "Personne, famille ou collectivité contribuant à une expression d’une œuvre en supervisant les aspects techniques d’une séance d’enregistrement sonore ou vidéo."@fr ;
    rdakit:toolkitLabel "recording engineer"@en,
        "ingeniero de grabación"@es,
        "ingénieur du son"@fr ;
    reg:hasSubproperty <http://rdaregistry.info/Elements/e/object/P20050> ;
    reg:hasUnconstrained <http://rdaregistry.info/Elements/u/P60395> ;
    reg:lexicalAlias <http://rdaregistry.info/Elements/e/recordingEngineer.en> ;
    reg:name "recordingEngineer"@en ;
    reg:status <http://metadataregistry.org/uri/RegStatus/1001> ;
    rdfs:domain <http://rdaregistry.info/Elements/c/C10006> ;
    rdfs:isDefinedBy <http://rdaregistry.info/Elements/e/> ;
    rdfs:subPropertyOf <http://rdaregistry.info/Elements/e/P20292> ;
    skos:definition "Relates an expression to an audio engineer contributing to the audio content of an expression by supervising the technical aspects of a recording session."@en .

<http://rdaregistry.info/Elements/e/P20052> a rdf:Property ;
    rdfs:label "has recordist"@en ;
    rdakit:instructionNumber "18.5" ;
    rdakit:toolkitDefinition "An agent contributing to an expression of a work by using a recording device to capture sound and/or video during a recording session, including field recordings of natural sounds, folkloric events, music, etc."@en,
        "Una persona, familia o entidad corporativa que contribuye a una expresión de una obra utilizando un mecanismo de grabación para capturar sonido y/o video durante una sesión de grabación, incluyendo grabación de sonidos naturales, eventos folclóricos, música, etc."@es,
        "Personne, famille ou collectivité contribuant à une expression d’une œuvre en utilisant un appareil d’enregistrement pour capter le son et/ou la vidéo durant une séance d’enregistrement, y compris les enregistrements de terrain de sons naturels, de prestations folkloriques, de musique, etc."@fr ;
    rdakit:toolkitLabel "recordist"@en,
        "técnico de grabación"@es,
        "opérateur d’enregistrement"@fr ;
    reg:hasSubproperty <http://rdaregistry.info/Elements/e/object/P20052> ;
    reg:hasUnconstrained <http://rdaregistry.info/Elements/u/P60397> ;
    reg:lexicalAlias <http://rdaregistry.info/Elements/e/recordist.en> ;
    reg:name "recordist"@en ;
    reg:status <http://metadataregistry.org/uri/RegStatus/1001> ;
    rdfs:domain <http://rdaregistry.info/Elements/c/C10006> ;
    rdfs:isDefinedBy <http://rdaregistry.info/Elements/e/> ;
    rdfs:subPropertyOf <http://rdaregistry.info/Elements/e/P20053> ;
    skos:definition "Relates an expression to an agent contributing to an expression of a work by using a recording device to capture sound and/or video during a recording session, including field recordings of natural sounds, folkloric events, music, etc."@en .

<http://rdaregistry.info/Elements/e/P20054> a rdf:Property ;
    rdfs:label "has presenter"@en ;
    rdakit:instructionNumber "18.5" ;
    rdakit:toolkitDefinition "An agent mentioned in an \"X presents:\" credit for moving image materials and who is probably associated with production, finance, or distribution in some way."@en,
        "Un intérprete que contribuye a una expresión de una obra dirigiendo un programa (a menudo una transmisión) que incluye otros invitados, intérpretes, etc., (por ej., presentadores de programas de debates).  "@es,
        "Personne, famille ou collectivité mentionnée dans un générique d’images animées sous la forme « X présente » et qui est probablement associée d’une façon quelconque à la production, au financement ou à la distribution."@fr ;
    rdakit:toolkitLabel "presenter"@en,
        "presentador"@es,
        "présentateur"@fr ;
    reg:hasSubproperty <http://rdaregistry.info/Elements/e/object/P20054> ;
    reg:hasUnconstrained <http://rdaregistry.info/Elements/u/P60419> ;
    reg:lexicalAlias <http://rdaregistry.info/Elements/e/presenter.en> ;
    reg:name "presenter"@en ;
    reg:status <http://metadataregistry.org/uri/RegStatus/1001> ;
    rdfs:domain <http://rdaregistry.info/Elements/c/C10006> ;
    rdfs:isDefinedBy <http://rdaregistry.info/Elements/e/> ;
    rdfs:subPropertyOf <http://rdaregistry.info/Elements/e/P20053> ;
    skos:definition "Relates an expression to an agent mentioned in an \"X presents:\" credit for moving image materials and who is probably associated with production, finance, or distribution in some way."@en .

<http://rdaregistry.info/Elements/e/P20055> a rdf:Property ;
    rdfs:label "has editor of moving image work"@en ;
    rdakit:instructionNumber "18.5" ;
    rdakit:toolkitDefinition "An agent responsible for assembling, arranging, and trimming film, video, or other moving image formats, including both visual and audio aspects."@en,
        "Una persona, familia o entidad corporativa responsable de unir, componer y recortar película cinematográfica, video u otros formatos de imágenes en movimiento, incluyendo tanto aspectos visuales como de sonido."@es,
        "Personne, famille ou collectivité responsable de l’assemblage, de l’arrangement et du découpage de film, de vidéo ou d’autres formats d’images animées, y compris les aspects visuels et sonores."@fr ;
    rdakit:toolkitLabel "editor of moving image work"@en,
        "montador"@es,
        "monteur d’œuvre d’images animées"@fr ;
    reg:hasSubproperty <http://rdaregistry.info/Elements/e/object/P20055> ;
    reg:hasUnconstrained <http://rdaregistry.info/Elements/u/P60422> ;
    reg:lexicalAlias <http://rdaregistry.info/Elements/e/editorOfMovingImageWork.en> ;
    reg:name "editorOfMovingImageWork"@en ;
    reg:status <http://metadataregistry.org/uri/RegStatus/1001> ;
    rdfs:domain <http://rdaregistry.info/Elements/c/C10006> ;
    rdfs:isDefinedBy <http://rdaregistry.info/Elements/e/> ;
    rdfs:subPropertyOf <http://rdaregistry.info/Elements/e/P20053> ;
    skos:definition "Relates an expression to an agent responsible for assembling, arranging, and trimming film, video, or other moving image formats, including both visual and audio aspects."@en .

<http://rdaregistry.info/Elements/e/P20056> a rdf:Property ;
    rdfs:label "has production designer"@en ;
    rdakit:instructionNumber "18.5" ;
    rdakit:toolkitDefinition "An agent responsible for designing the overall visual appearance of a moving image production."@en,
        "Una persona, familia o entidad corporativa responsable del diseño de la apariencia visual general de una producción de una imagen en movimiento."@es,
        "Personne, famille ou collectivité responsable de concevoir l’aspect visuel global d’une production d’images animées."@fr ;
    rdakit:toolkitLabel "production designer"@en,
        "diseñador de producción"@es,
        "chef décorateur"@fr ;
    reg:hasSubproperty <http://rdaregistry.info/Elements/e/object/P20056> ;
    reg:hasUnconstrained <http://rdaregistry.info/Elements/u/P60437> ;
    reg:lexicalAlias <http://rdaregistry.info/Elements/e/productionDesigner.en> ;
    reg:name "productionDesigner"@en ;
    reg:status <http://metadataregistry.org/uri/RegStatus/1001> ;
    rdfs:domain <http://rdaregistry.info/Elements/c/C10006> ;
    rdfs:isDefinedBy <http://rdaregistry.info/Elements/e/> ;
    rdfs:subPropertyOf <http://rdaregistry.info/Elements/e/P20053> ;
    skos:definition "Relates an expression to an agent responsible for designing the overall visual appearance of a moving image production."@en .

<http://rdaregistry.info/Elements/e/P20058> a rdf:Property ;
    rdfs:label "has minute taker"@en ;
    rdakit:instructionNumber "18.5" ;
    rdakit:toolkitDefinition "An agent responsible for recording the minutes of a meeting."@en,
        "Una persona, familia o entidad corporativa responsable de registrar las actas de una reunión."@es,
        "Personne, famille ou collectivité responsable de rédiger le procès-verbal d’une réunion."@fr ;
    rdakit:toolkitLabel "minute taker"@en,
        "secretario de actas"@es,
        "procès-verbaliste"@fr ;
    reg:hasSubproperty <http://rdaregistry.info/Elements/e/object/P20058> ;
    reg:hasUnconstrained <http://rdaregistry.info/Elements/u/P60446> ;
    reg:lexicalAlias <http://rdaregistry.info/Elements/e/minuteTaker.en> ;
    reg:name "minuteTaker"@en ;
    reg:status <http://metadataregistry.org/uri/RegStatus/1001> ;
    rdfs:domain <http://rdaregistry.info/Elements/c/C10006> ;
    rdfs:isDefinedBy <http://rdaregistry.info/Elements/e/> ;
    rdfs:subPropertyOf <http://rdaregistry.info/Elements/e/P20053> ;
    skos:definition "Relates an expression to an agent responsible for recording the minutes of a meeting."@en .

<http://rdaregistry.info/Elements/e/P20060> a rdf:Property ;
    rdfs:label "is adapted as radio program (expression)"@en ;
    rdakit:instructionNumber "24.5" ;
    rdakit:toolkitDefinition "A radio program based on a source expression."@en,
        "Un programa de radio basado en la expresión fuente."@es,
        "Émission de radio basée sur l’expression source."@fr ;
    rdakit:toolkitLabel "adapted as radio program (expression)"@en,
        "adaptada como programa de radio (expresión)"@es,
        "adapté en émission de radio (expression)"@fr ;
    reg:hasSubproperty <http://rdaregistry.info/Elements/e/object/P20060> ;
    reg:hasUnconstrained <http://rdaregistry.info/Elements/u/P60174> ;
    reg:lexicalAlias <http://rdaregistry.info/Elements/e/adaptedAsRadioProgramExpression.en> ;
    reg:name "adaptedAsRadioProgramExpression"@en ;
    reg:status <http://metadataregistry.org/uri/RegStatus/1001> ;
    rdfs:domain <http://rdaregistry.info/Elements/c/C10006> ;
    rdfs:isDefinedBy <http://rdaregistry.info/Elements/e/> ;
    rdfs:subPropertyOf <http://rdaregistry.info/Elements/e/P20153> ;
    skos:definition "Relates an expression to a radio program based on a source expression."@en .

<http://rdaregistry.info/Elements/e/P20061> a rdf:Property ;
    rdfs:label "has form of tactile notation"@en,
        "har form av taktil notation"@sv ;
    rdakit:instructionNumber "7.13.4" ;
    rdakit:toolkitDefinition "A set of characters or symbols used to express the content of an expression in a form that can be perceived through touch."@en,
        "Un conjunto de caracteres y/o símbolos utilizados para expresar el contenido de un recurso en tal forma que se pueda percibir mediante el tacto."@es,
        "Ensemble de signes et/ou de symboles utilisés pour exprimer le contenu d’une ressource sous une forme perceptible au toucher."@fr ;
    rdakit:toolkitLabel "form of tactile notation"@en,
        "forma de notación táctil"@es,
        "forme de la notation tactile"@fr,
        "form av taktil notation"@sv ;
    reg:hasUnconstrained <http://rdaregistry.info/Elements/u/P60318> ;
    reg:lexicalAlias <http://rdaregistry.info/Elements/e/formOfTactileNotation.en> ;
    reg:name "formOfTactileNotation"@en ;
    reg:status <http://metadataregistry.org/uri/RegStatus/1001> ;
    rdfs:domain <http://rdaregistry.info/Elements/c/C10006> ;
    rdfs:isDefinedBy <http://rdaregistry.info/Elements/e/> ;
    rdfs:subPropertyOf <http://rdaregistry.info/Elements/e/P20062> ;
    skos:definition "Relates an expression to a set of characters or symbols used to express the content of an expression in a form that can be perceived through touch."@en .

<http://rdaregistry.info/Elements/e/P20063> a rdf:Property ;
    rdfs:label "has form of notated movement"@en ;
    rdakit:instructionNumber "7.13.5" ;
    rdakit:toolkitDefinition "A set of characters or symbols used to express movement content of an expression."@en,
        "Un conjunto de caracteres y/o símbolos usados para expresar el contenido de movimientos de un recurso."@es,
        "Ensemble de signes et/ou de caractères utilisés pour exprimer le contenu du mouvement d’une ressource."@fr ;
    rdakit:toolkitLabel "form of notated movement"@en,
        "forma de notación de movimientos"@es,
        "forme de la notation du mouvement"@fr ;
    reg:hasUnconstrained <http://rdaregistry.info/Elements/u/P60320> ;
    reg:lexicalAlias <http://rdaregistry.info/Elements/e/formOfNotatedMovement.en> ;
    reg:name "formOfNotatedMovement"@en ;
    reg:status <http://metadataregistry.org/uri/RegStatus/1001> ;
    rdfs:domain <http://rdaregistry.info/Elements/c/C10006> ;
    rdfs:isDefinedBy <http://rdaregistry.info/Elements/e/> ;
    rdfs:subPropertyOf <http://rdaregistry.info/Elements/e/P20062> ;
    skos:definition "Relates an expression to a set of characters or symbols used to express movement content of an expression."@en .

<http://rdaregistry.info/Elements/e/P20064> a rdf:Property ;
    rdfs:label "has form of musical notation"@en,
        "har form av musiknotation"@sv ;
    rdakit:instructionNumber "7.13.3" ;
    rdakit:toolkitDefinition "A set of characters or symbols used to express musical content of an expression."@en,
        "Un conjunto de caracteres y/o símbolos utilizados para expresar el contenido musical de un recurso."@es,
        "Ensemble de signes et/ou de symboles utilisés pour exprimer le contenu musical d’une ressource"@fr ;
    rdakit:toolkitLabel "form of musical notation"@en,
        "forma de la notación musical"@es,
        "forme de la notation musicale"@fr,
        "form av musiknotation"@sv ;
    reg:hasUnconstrained <http://rdaregistry.info/Elements/u/P60321> ;
    reg:lexicalAlias <http://rdaregistry.info/Elements/e/formOfMusicalNotation.en> ;
    reg:name "formOfMusicalNotation"@en ;
    reg:status <http://metadataregistry.org/uri/RegStatus/1001> ;
    rdfs:domain <http://rdaregistry.info/Elements/c/C10006> ;
    rdfs:isDefinedBy <http://rdaregistry.info/Elements/e/> ;
    rdfs:subPropertyOf <http://rdaregistry.info/Elements/e/P20062> ;
    skos:definition "Relates an expression to a set of characters or symbols used to express musical content of an expression."@en .

<http://rdaregistry.info/Elements/e/P20065> a rdf:Property ;
    rdfs:label "has script"@en ;
    rdakit:instructionNumber "7.13.2" ;
    rdakit:toolkitDefinition "A set of characters and/or symbols used to express written language content of an expression."@en,
        "Un conjunto de caracteres y/o símbolos utilizados para expresar en lengua escrita el contenido de un recurso."@es,
        "Ensemble de caractères et/ou de symboles utilisé pour exprimer le contenu linguistique écrit d’une ressource."@fr ;
    rdakit:toolkitLabel "script"@en,
        "escritura"@es,
        "écriture"@fr ;
    reg:hasUnconstrained <http://rdaregistry.info/Elements/u/P60322> ;
    reg:lexicalAlias <http://rdaregistry.info/Elements/e/script.en> ;
    reg:name "script"@en ;
    reg:status <http://metadataregistry.org/uri/RegStatus/1001> ;
    rdfs:domain <http://rdaregistry.info/Elements/c/C10006> ;
    rdfs:isDefinedBy <http://rdaregistry.info/Elements/e/> ;
    rdfs:subPropertyOf <http://rdaregistry.info/Elements/e/P20062> ;
    skos:definition "Relates an expression to a set of characters or symbols used to express written language content of an expression."@en .

<http://rdaregistry.info/Elements/e/P20066> a rdf:Property ;
    rdfs:label "is adapted as television program (expression)"@en ;
    rdakit:instructionNumber "24.5" ;
    rdakit:toolkitDefinition "A television program based on a source expression."@en,
        "Un programa de televisión basado en la expresión fuente."@es,
        "Émission de télévision basée sur l’expression source."@fr ;
    rdakit:toolkitLabel "adapted as television program (expression)"@en,
        "adaptada como programa de televisión (expresión)"@es,
        "adapté en émission de télévision (expression)"@fr ;
    reg:hasSubproperty <http://rdaregistry.info/Elements/e/object/P20066> ;
    reg:hasUnconstrained <http://rdaregistry.info/Elements/u/P60354> ;
    reg:lexicalAlias <http://rdaregistry.info/Elements/e/adaptedAsTelevisionProgramExpression.en> ;
    reg:name "adaptedAsTelevisionProgramExpression"@en ;
    reg:status <http://metadataregistry.org/uri/RegStatus/1001> ;
    rdfs:domain <http://rdaregistry.info/Elements/c/C10006> ;
    rdfs:isDefinedBy <http://rdaregistry.info/Elements/e/> ;
    rdfs:subPropertyOf <http://rdaregistry.info/Elements/e/P20153> ;
    skos:definition "Relates an expression to a television program based on a source expression."@en .

<http://rdaregistry.info/Elements/e/P20067> a rdf:Property ;
    rdfs:label "is adapted as video (expression)"@en ;
    rdakit:instructionNumber "24.5" ;
    rdakit:toolkitDefinition "A video based on a source expression."@en,
        "Un video basado en la expresión fuente."@es,
        "Vidéo basée sur l’expression source."@fr ;
    rdakit:toolkitLabel "adapted as video (expression)"@en,
        "adaptada como video (expresión)"@es,
        "adapté en vidéo (expression)"@fr ;
    reg:hasSubproperty <http://rdaregistry.info/Elements/e/object/P20067> ;
    reg:hasUnconstrained <http://rdaregistry.info/Elements/u/P60361> ;
    reg:lexicalAlias <http://rdaregistry.info/Elements/e/adaptedAsVideoExpression.en> ;
    reg:name "adaptedAsVideoExpression"@en ;
    reg:status <http://metadataregistry.org/uri/RegStatus/1001> ;
    rdfs:domain <http://rdaregistry.info/Elements/c/C10006> ;
    rdfs:isDefinedBy <http://rdaregistry.info/Elements/e/> ;
    rdfs:subPropertyOf <http://rdaregistry.info/Elements/e/P20153> ;
    skos:definition "Relates an expression to a video based on a source expression."@en .

<http://rdaregistry.info/Elements/e/P20068> a rdf:Property ;
    rdfs:label "has writer of added lyrics"@en ;
    rdakit:instructionNumber "18.5" ;
    rdakit:seeAlso <http://rdaregistry.info/Elements/w/P10204> ;
    rdakit:toolkitDefinition "A writer of words added to an expression of a musical work."@en,
        "Un autor que agrega palabras a una expresión de una obra musical."@es,
        "Auteur de paroles ajoutées à une expression d’une œuvre musicale."@fr ;
    rdakit:toolkitLabel "writer of added lyrics"@en,
        "autor de letra adicional"@es,
        "auteur de paroles ajoutées"@fr ;
    reg:hasSubproperty <http://rdaregistry.info/Elements/e/object/P20068> ;
    reg:hasUnconstrained <http://rdaregistry.info/Elements/u/P60371> ;
    reg:lexicalAlias <http://rdaregistry.info/Elements/e/writerOfAddedLyrics.en> ;
    reg:name "writerOfAddedLyrics"@en ;
    reg:status <http://metadataregistry.org/uri/RegStatus/1001> ;
    rdfs:domain <http://rdaregistry.info/Elements/c/C10006> ;
    rdfs:isDefinedBy <http://rdaregistry.info/Elements/e/> ;
    rdfs:subPropertyOf <http://rdaregistry.info/Elements/e/P20030> ;
    skos:definition "Relates an expression to a writer of words added to an expression of a musical work."@en ;
    skos:scopeNote "Writing of lyrics in collaboration with a composer to form an original work is excluded."@en .

<http://rdaregistry.info/Elements/e/P20070> a rdf:Property ;
    rdfs:label "has voice actor"@en ;
    rdakit:instructionNumber "18.5" ;
    rdakit:toolkitDefinition "An actor contributing to an expression of a work by providing the voice for characters in radio and audio productions and for animated characters in moving image works, as well as by providing voice-overs in radio and television commercials, dubbed resources, etc."@en,
        "Un actor que contribuye a una expresión de una obra proporcionando la voz de los personajes en radio y producciones de sonido y de personajes animados en obras de imágenes en movimiento, al igual que proporcionando voces sobrepuestas en comerciales de radio y televisión, recursos de doblaje, etc."@es,
        "Acteur contribuant à une expression d’une œuvre en prêtant sa voix à des personnages dans des productions radiophoniques et audio et à des personnages animés dans des œuvres d’images animées, de même qu’en prêtant sa voix hors champ dans des messages publicitaires à la radio et à la télévision, du doublage, etc."@fr ;
    rdakit:toolkitLabel "voice actor"@en,
        "actor de voz"@es,
        "voix"@fr ;
    reg:hasSubproperty <http://rdaregistry.info/Elements/e/object/P20070> ;
    reg:hasUnconstrained <http://rdaregistry.info/Elements/u/P60152> ;
    reg:lexicalAlias <http://rdaregistry.info/Elements/e/voiceActor.en> ;
    reg:name "voiceActor"@en ;
    reg:status <http://metadataregistry.org/uri/RegStatus/1001> ;
    rdfs:domain <http://rdaregistry.info/Elements/c/C10006> ;
    rdfs:isDefinedBy <http://rdaregistry.info/Elements/e/> ;
    rdfs:subPropertyOf <http://rdaregistry.info/Elements/e/P20012> ;
    skos:definition "Relates an expression to an actor contributing to an expression of a work by providing the voice for characters in radio and audio productions and for animated characters in moving image works, as well as by providing voice-overs in radio and television commercials, dubbed expressions, etc."@en .

<http://rdaregistry.info/Elements/e/P20073> a rdf:Property ;
    rdfs:label "is dramatized as (expression)"@en ;
    rdakit:instructionNumber "24.5" ;
    rdakit:toolkitDefinition "An expression of a dramatic work adapted from a source expression."@en,
        "Una expresión de una obra dramática adaptada de la expresión fuente."@es,
        "Expression d’une œuvre théâtrale adaptée de l’expression source."@fr ;
    rdakit:toolkitLabel "dramatized as (expression)"@en,
        "dramatizada como (expresión)"@es,
        "adapté au théâtre comme (expression)"@fr ;
    reg:hasSubproperty <http://rdaregistry.info/Elements/e/object/P20073> ;
    reg:hasUnconstrained <http://rdaregistry.info/Elements/u/P60088> ;
    reg:lexicalAlias <http://rdaregistry.info/Elements/e/dramatizedAsExpression.en> ;
    reg:name "dramatizedAsExpression"@en ;
    reg:status <http://metadataregistry.org/uri/RegStatus/1001> ;
    rdfs:domain <http://rdaregistry.info/Elements/c/C10006> ;
    rdfs:isDefinedBy <http://rdaregistry.info/Elements/e/> ;
    rdfs:subPropertyOf <http://rdaregistry.info/Elements/e/P20153> ;
    skos:definition "Relates an expression to an expression of a dramatic work adapted from a source expression."@en .

<http://rdaregistry.info/Elements/e/P20074> a rdf:Property ;
    rdfs:label "is contained in (expression)"@en ;
    rdakit:instructionNumber "24.5" ;
    rdakit:toolkitDefinition "An expression of a larger work of which the expression is a discrete component."@en,
        "Una expresión de una obra mayor de la cual una parte es un componente separado."@es,
        "Expression d’une œuvre plus vaste dont l’expression est une composante distincte."@fr ;
    rdakit:toolkitLabel "contained in (expression)"@en,
        "contenida en (expresión)"@es,
        "contenu dans (expression)"@fr ;
    reg:hasSubproperty <http://rdaregistry.info/Elements/e/object/P20074> ;
    reg:hasUnconstrained <http://rdaregistry.info/Elements/u/P60101> ;
    reg:lexicalAlias <http://rdaregistry.info/Elements/e/containedInExpression.en> ;
    reg:name "containedInExpression"@en ;
    reg:status <http://metadataregistry.org/uri/RegStatus/1001> ;
    rdfs:domain <http://rdaregistry.info/Elements/c/C10006> ;
    rdfs:isDefinedBy <http://rdaregistry.info/Elements/e/> ;
    rdfs:subPropertyOf <http://rdaregistry.info/Elements/e/P20236> ;
    skos:definition "Relates an expression to an expression of a larger work of which the expression is a discrete component."@en .

<http://rdaregistry.info/Elements/e/P20075> a rdf:Property ;
    rdfs:label "is replaced in part by (expression)"@en ;
    rdakit:instructionNumber "24.5" ;
    rdakit:toolkitDefinition "An expression of a later work used in part in place of an earlier expression usually because the later work contains updated or new information that makes part of the earlier expression obsolete."@en,
        "Una expresión de una obra anterior cuyo contenido ha sido reemplazado parcialmente por una expresión posterior, generalmente porque la obra posterior contiene información actualizada o nueva que hace obsoleta la expresión anterior."@es,
        "Expression d’une œuvre ultérieure utilisée en partie à la place d’une expression antérieure, généralement parce que l’œuvre ultérieure contient de l’information nouvelle ou mise à jour qui rend une partie de l’expression antérieure obsolète."@fr ;
    rdakit:toolkitLabel "replaced in part by (expression)"@en,
        "reemplazo en parte de (expresión)"@es,
        "remplacé en partie par (expression)"@fr ;
    reg:hasSubproperty <http://rdaregistry.info/Elements/e/object/P20075> ;
    reg:hasUnconstrained <http://rdaregistry.info/Elements/u/P60103> ;
    reg:lexicalAlias <http://rdaregistry.info/Elements/e/replacedInPartByExpression.en> ;
    reg:name "replacedInPartByExpression"@en ;
    reg:status <http://metadataregistry.org/uri/RegStatus/1001> ;
    rdfs:domain <http://rdaregistry.info/Elements/c/C10006> ;
    rdfs:isDefinedBy <http://rdaregistry.info/Elements/e/> ;
    rdfs:subPropertyOf <http://rdaregistry.info/Elements/e/P20169> ;
    skos:definition "Relates an expression to an expression of a later work used in part in place of an earlier expression usually because the later work contains updated or new information that makes part of the earlier expression obsolete."@en ;
    skos:scopeNote "This relationship applies generally to single-part units, multipart monographs, and integrating resources."@en .

<http://rdaregistry.info/Elements/e/P20076> a rdf:Property ;
    rdfs:label "is replaced by (expression)"@en ;
    rdakit:instructionNumber "24.5" ;
    rdakit:toolkitDefinition "An expression of a later work used in place of an earlier expression, usually because the later work contains updated or new information that makes the earlier expression obsolete."@en,
        "Una expresión de una obra anterior cuyo contenido ha sido reemplazado por una expresión posterior, generalmente porque la obra posterior contiene información actualizada o nueva que hace obsoleta la expresión anterior."@es,
        "Expression d’une œuvre ultérieure utilisée à la place d’une expression antérieure, généralement parce que l’œuvre ultérieure contient de l’information nouvelle ou mise à jour qui rend l’expression antérieure obsolète."@fr ;
    rdakit:toolkitLabel "replaced by (expression)"@en,
        "reemplazo de (expresión)"@es,
        "remplacé par (expression)"@fr ;
    reg:hasSubproperty <http://rdaregistry.info/Elements/e/object/P20076> ;
    reg:hasUnconstrained <http://rdaregistry.info/Elements/u/P60104> ;
    reg:lexicalAlias <http://rdaregistry.info/Elements/e/replacedByExpression.en> ;
    reg:name "replacedByExpression"@en ;
    reg:status <http://metadataregistry.org/uri/RegStatus/1001> ;
    rdfs:domain <http://rdaregistry.info/Elements/c/C10006> ;
    rdfs:isDefinedBy <http://rdaregistry.info/Elements/e/> ;
    rdfs:subPropertyOf <http://rdaregistry.info/Elements/e/P20169> ;
    skos:definition "Relates an expression to an expression of a later work used in place of an earlier expression, usually because the later work contains updated or new information that makes the earlier expression obsolete."@en ;
    skos:scopeNote "This relationship applies generally to single-part units, multipart monographs, and integrating resources."@en .

<http://rdaregistry.info/Elements/e/P20077> a rdf:Property ;
    rdfs:label "is adapted in verse as (expression)"@en ;
    rdakit:instructionNumber "24.5" ;
    rdakit:toolkitDefinition "An expression of a literary composition in verse form adapted from a source expression."@en,
        "Una expresión de una obra que fue adaptada como una composición literaria en forma de verso."@es,
        "Expression d’une composition littéraire en vers adaptée de l’expression source."@fr ;
    rdakit:toolkitLabel "adapted in verse as (expression)"@en,
        "adaptación en verso de (expresión)"@es,
        "adapté en vers comme (expression)"@fr ;
    reg:hasSubproperty <http://rdaregistry.info/Elements/e/object/P20077> ;
    reg:hasUnconstrained <http://rdaregistry.info/Elements/u/P60106> ;
    reg:lexicalAlias <http://rdaregistry.info/Elements/e/adaptedInVerseAsExpression.en> ;
    reg:name "adaptedInVerseAsExpression"@en ;
    reg:status <http://metadataregistry.org/uri/RegStatus/1001> ;
    rdfs:domain <http://rdaregistry.info/Elements/c/C10006> ;
    rdfs:isDefinedBy <http://rdaregistry.info/Elements/e/> ;
    rdfs:subPropertyOf <http://rdaregistry.info/Elements/e/P20153> ;
    skos:definition "Relates an expression to an expression of a literary composition in verse form adapted from a source expression."@en .

<http://rdaregistry.info/Elements/e/P20078> a rdf:Property ;
    rdfs:label "is dubbed version of"@en ;
    rdakit:instructionNumber "24.5" ;
    rdakit:toolkitDefinition "An expression of a moving image work in which spoken dialogue has been translated into a language different from that of the original work."@en,
        "Una expresión de una obra de imagen en movimiento en la cual el diálogo hablado se ha traducido a una lengua diferente de la de la obra original."@es,
        "Expression d’une œuvre d’images animées dans laquelle les dialogues parlés ont été traduits dans une langue différente de celle de l’œuvre d’origine."@fr ;
    rdakit:toolkitLabel "dubbed version of"@en,
        "versión doblada de"@es,
        "version doublée de"@fr ;
    reg:hasSubproperty <http://rdaregistry.info/Elements/e/object/P20078> ;
    reg:hasUnconstrained <http://rdaregistry.info/Elements/u/P60111> ;
    reg:lexicalAlias <http://rdaregistry.info/Elements/e/dubbedVersionOf.en> ;
    reg:name "dubbedVersionOf"@en ;
    reg:status <http://metadataregistry.org/uri/RegStatus/1001> ;
    rdfs:domain <http://rdaregistry.info/Elements/c/C10006> ;
    rdfs:isDefinedBy <http://rdaregistry.info/Elements/e/> ;
    rdfs:subPropertyOf <http://rdaregistry.info/Elements/e/P20141> ;
    skos:definition "Relates an expression to an expression of a moving image work in which spoken dialogue has been translated into a language different from that of the original work."@en .

<http://rdaregistry.info/Elements/e/P20079> a rdf:Property ;
    rdfs:label "is dubbed version"@en ;
    rdakit:instructionNumber "24.5" ;
    rdakit:toolkitDefinition "An expression of a moving image work that translates spoken dialogue of the original work into a different language."@en,
        "Una expresión de una obra de imagen en movimiento que traduce el diálogo hablado de la obra original en una lengua diferente."@es,
        "Expression d’une œuvre d’images animées qui traduit les dialogues parlés de l’œuvre d’origine dans une langue différente."@fr ;
    rdakit:toolkitLabel "dubbed version"@en,
        "versión doblada"@es,
        "version doublée"@fr ;
    reg:hasSubproperty <http://rdaregistry.info/Elements/e/object/P20079> ;
    reg:hasUnconstrained <http://rdaregistry.info/Elements/u/P60112> ;
    reg:lexicalAlias <http://rdaregistry.info/Elements/e/dubbedVersion.en> ;
    reg:name "dubbedVersion"@en ;
    reg:status <http://metadataregistry.org/uri/RegStatus/1001> ;
    rdfs:domain <http://rdaregistry.info/Elements/c/C10006> ;
    rdfs:isDefinedBy <http://rdaregistry.info/Elements/e/> ;
    rdfs:subPropertyOf <http://rdaregistry.info/Elements/e/P20171> ;
    skos:definition "Relates an expression to an expression of a moving image work that translates spoken dialogue of the original work into a different language."@en .

<http://rdaregistry.info/Elements/e/P20080> a rdf:Property ;
    rdfs:label "is cadenza (expression)"@en ;
    rdakit:instructionNumber "24.5" ;
    rdakit:toolkitDefinition "An expression of a musical work consisting of an ornamental passage for a soloist, added to a musical work such as a concerto, either by the same or a different composer."@en,
        "Una expresión de una obra musical que consiste en un pasaje ornamental para un solista, añadida a una obra musical como un concierto, por igual o diferente compositor."@es,
        "Expression d’une œuvre musicale consistant en un passage ornemental pour soliste, ajouté à une œuvre musicale telle qu’un concerto, soit par le même compositeur, soit par un compositeur différent."@fr ;
    rdakit:toolkitLabel "cadenza (expression)"@en,
        "cadencia (expresión)"@es,
        "cadence (expression)"@fr ;
    reg:hasSubproperty <http://rdaregistry.info/Elements/e/object/P20080> ;
    reg:hasUnconstrained <http://rdaregistry.info/Elements/u/P60113> ;
    reg:lexicalAlias <http://rdaregistry.info/Elements/e/cadenzaExpression.en> ;
    reg:name "cadenzaExpression"@en ;
    reg:status <http://metadataregistry.org/uri/RegStatus/1001> ;
    rdfs:domain <http://rdaregistry.info/Elements/c/C10006> ;
    rdfs:isDefinedBy <http://rdaregistry.info/Elements/e/> ;
    rdfs:subPropertyOf <http://rdaregistry.info/Elements/e/P20105> ;
    skos:definition "Relates an expression to an expression of a musical work consisting of an ornamental passage for a soloist, added to a musical work such as a concerto, either by the same or a different composer."@en .

<http://rdaregistry.info/Elements/e/P20081> a rdf:Property ;
    rdfs:label "is variations based on (expression)"@en ;
    rdakit:instructionNumber "24.5" ;
    rdakit:toolkitDefinition "An expression of a musical work from which melodic, thematic, or harmonic material is taken to form a discrete theme, which is repeated one or more times with subsequent modifications."@en,
        "Una expresión de una obra musical de la cual se toma el material melódico, temático o armónico para formar un tema separado, el cual es repetido una o más veces con modificaciones subsecuentes."@es,
        "Expression d’une œuvre musicale d’où est tirée de la matière mélodique, thématique ou harmonique pour former un thème distinct, qui est répété une ou plusieurs fois avec des modifications subséquentes."@fr ;
    rdakit:toolkitLabel "variations based on (expression)"@en,
        "variaciones basadas en (expresión)"@es,
        "variations basées sur (expression)"@fr ;
    reg:hasSubproperty <http://rdaregistry.info/Elements/e/object/P20081> ;
    reg:hasUnconstrained <http://rdaregistry.info/Elements/u/P60114> ;
    reg:lexicalAlias <http://rdaregistry.info/Elements/e/variationsBasedOnExpression.en> ;
    reg:name "variationsBasedOnExpression"@en ;
    reg:status <http://metadataregistry.org/uri/RegStatus/1001> ;
    rdfs:domain <http://rdaregistry.info/Elements/c/C10006> ;
    rdfs:isDefinedBy <http://rdaregistry.info/Elements/e/> ;
    rdfs:subPropertyOf <http://rdaregistry.info/Elements/e/P20204> ;
    skos:definition "Relates an expression to an expression of a musical work from which melodic, thematic, or harmonic material is taken to form a discrete theme, which is repeated one or more times with subsequent modifications."@en .

<http://rdaregistry.info/Elements/e/P20082> a rdf:Property ;
    rdfs:label "is modified by variation as (expression)"@en ;
    rdakit:instructionNumber "24.5" ;
    rdakit:toolkitDefinition "An expression of a musical work in which melodic, thematic, or harmonic material taken from a source work forms a discrete theme, which is repeated one or more times with subsequent modifications."@en,
        "Una expresión de una obra musical en la cual el material melódico, temático o harmónico se toma de la obra fuente para formar un tema separado, el cual se repite una o mas veces con las subsecuentes modificaciones."@es,
        "Expression d’une œuvre musicale dans laquelle de la matière mélodique, thématique ou harmonique tirée de l’œuvre source forme un thème distinct qui est répété une ou plusieurs fois avec des modifications subséquentes."@fr ;
    rdakit:toolkitLabel "modified by variation as (expression)"@en,
        "modificada por variación como (expresión)"@es,
        "modifié par variation comme (expression)"@fr ;
    reg:hasSubproperty <http://rdaregistry.info/Elements/e/object/P20082> ;
    reg:hasUnconstrained <http://rdaregistry.info/Elements/u/P60115> ;
    reg:lexicalAlias <http://rdaregistry.info/Elements/e/modifiedByVariationAsExpression.en> ;
    reg:name "modifiedByVariationAsExpression"@en ;
    reg:status <http://metadataregistry.org/uri/RegStatus/1001> ;
    rdfs:domain <http://rdaregistry.info/Elements/c/C10006> ;
    rdfs:isDefinedBy <http://rdaregistry.info/Elements/e/> ;
    rdfs:subPropertyOf <http://rdaregistry.info/Elements/e/P20203> ;
    skos:definition "Relates an expression to an expression of a musical work in which melodic, thematic, or harmonic material taken from a source work forms a discrete theme, which is repeated one or more times with subsequent modifications."@en .

<http://rdaregistry.info/Elements/e/P20083> a rdf:Property ;
    rdfs:label "is cadenza composed for (expression)"@en ;
    rdakit:instructionNumber "24.5" ;
    rdakit:toolkitDefinition "An expression of a musical work such as a concerto for which an ornamental passage for a soloist has been composed, either by the same or a different composer."@en,
        "Una expresión de una obra musical tal como un concierto para el cual se ha compuesto un pasaje ornamental para solista, ya sea por el mismo o diferente compositor."@es,
        "Expression d’une œuvre musicale telle qu’un concerto pour laquelle un passage ornemental pour soliste a été composé, soit par le même compositeur, soit par un compositeur différent."@fr ;
    rdakit:toolkitLabel "cadenza composed for (expression)"@en,
        "cadencia compuesta para (expresión)"@es,
        "cadence composée pour (expression)"@fr ;
    reg:hasSubproperty <http://rdaregistry.info/Elements/e/object/P20083> ;
    reg:hasUnconstrained <http://rdaregistry.info/Elements/u/P60116> ;
    reg:lexicalAlias <http://rdaregistry.info/Elements/e/cadenzaComposedForExpression.en> ;
    reg:name "cadenzaComposedForExpression"@en ;
    reg:status <http://metadataregistry.org/uri/RegStatus/1001> ;
    rdfs:domain <http://rdaregistry.info/Elements/c/C10006> ;
    rdfs:isDefinedBy <http://rdaregistry.info/Elements/e/> ;
    rdfs:subPropertyOf <http://rdaregistry.info/Elements/e/P20192> ;
    skos:definition "Relates an expression to an expression of a musical work such as a concerto for which an ornamental passage for a soloist has been composed, either by the same or a different composer."@en .

<http://rdaregistry.info/Elements/e/P20084> a rdf:Property ;
    rdfs:label "is libretto for (expression)"@en ;
    rdakit:instructionNumber "24.5" ;
    rdakit:toolkitDefinition "An expression of a musical work such as an opera or other work for the musical stage, or an oratorio, that uses the text of a related work."@en,
        "Una expresión de una obra musical tal como una ópera u otra obra para representación musical, o un oratorio, que utiliza el texto de la obra relacionada."@es,
        "Expression d’une œuvre musicale telle qu’un opéra ou une autre œuvre pour la scène musicale, ou telle qu’un oratorio, qui utilise le texte de l’œuvre en relation."@fr ;
    rdakit:toolkitLabel "libretto for (expression)"@en,
        "libreto para (expresión)"@es,
        "livret pour (expression)"@fr ;
    reg:hasSubproperty <http://rdaregistry.info/Elements/e/object/P20084> ;
    reg:hasUnconstrained <http://rdaregistry.info/Elements/u/P60117> ;
    reg:lexicalAlias <http://rdaregistry.info/Elements/e/librettoForExpression.en> ;
    reg:name "librettoForExpression"@en ;
    reg:status <http://metadataregistry.org/uri/RegStatus/1001> ;
    rdfs:domain <http://rdaregistry.info/Elements/c/C10006> ;
    rdfs:isDefinedBy <http://rdaregistry.info/Elements/e/> ;
    rdfs:subPropertyOf <http://rdaregistry.info/Elements/e/P20100> ;
    skos:definition "Relates an expression to an expression of a musical work such as an opera or other work for the musical stage, or an oratorio, that uses the text of a related work."@en .

<http://rdaregistry.info/Elements/e/P20085> a rdf:Property ;
    rdfs:label "is incidental music (expression)"@en ;
    rdakit:instructionNumber "24.5" ;
    rdakit:toolkitDefinition "An expression of a musical work that that provides incidental music for a play or other spoken work for the stage."@en,
        "Una expresión de una obra musical que proporciona la música incidental para una obra de teatro u otra obra hablada para el escenario."@es,
        "Expression d’une œuvre musicale qui fournit la musique de scène pour une pièce de théâtre ou une autre œuvre parlée pour la scène."@fr ;
    rdakit:toolkitLabel "incidental music (expression)"@en,
        "música incidental (expresión)"@es,
        "musique de scène (expression)"@fr ;
    reg:hasSubproperty <http://rdaregistry.info/Elements/e/object/P20085> ;
    reg:hasUnconstrained <http://rdaregistry.info/Elements/u/P60118> ;
    reg:lexicalAlias <http://rdaregistry.info/Elements/e/incidentalMusicExpression.en> ;
    reg:name "incidentalMusicExpression"@en ;
    reg:status <http://metadataregistry.org/uri/RegStatus/1001> ;
    rdfs:domain <http://rdaregistry.info/Elements/c/C10006> ;
    rdfs:isDefinedBy <http://rdaregistry.info/Elements/e/> ;
    rdfs:subPropertyOf <http://rdaregistry.info/Elements/e/P20243> ;
    skos:definition "Relates an expression to an expression of a musical work that that provides incidental music for a play or other spoken work for the stage."@en .

<http://rdaregistry.info/Elements/e/P20086> a rdf:Property ;
    rdfs:label "is remade as (expression)"@en ;
    rdakit:instructionNumber "24.5" ;
    rdakit:toolkitDefinition "An expression of a new motion picture, radio program, television program, or video based on an earlier work."@en,
        "Una expresión de una película cinematográfica, programa radial, programa de televisión o video nuevo basada en una obra anterior."@es,
        "Expression d’un nouveau film, d’une nouvelle émission de radio, d’une nouvelle émission de télévision ou d’une nouvelle vidéo basée sur une œuvre antérieure."@fr ;
    rdakit:toolkitLabel "remade as (expression)"@en,
        "reproducida como (expresión)"@es,
        "repris comme (expression)"@fr ;
    reg:hasSubproperty <http://rdaregistry.info/Elements/e/object/P20086> ;
    reg:hasUnconstrained <http://rdaregistry.info/Elements/u/P60120> ;
    reg:lexicalAlias <http://rdaregistry.info/Elements/e/remadeAsExpression.en> ;
    reg:name "remadeAsExpression"@en ;
    reg:status <http://metadataregistry.org/uri/RegStatus/1001> ;
    rdfs:domain <http://rdaregistry.info/Elements/c/C10006> ;
    rdfs:isDefinedBy <http://rdaregistry.info/Elements/e/> ;
    rdfs:subPropertyOf <http://rdaregistry.info/Elements/e/P20203> ;
    skos:definition "Relates an expression to an expression of a motion picture, radio program, television program, or video based on an earlier work."@en .

<http://rdaregistry.info/Elements/e/P20087> a rdf:Property ;
    rdfs:label "is set to music as (expression)"@en ;
    rdakit:instructionNumber "24.5" ;
    rdakit:toolkitDefinition "An expression of a non-dramatic musical work, other than an oratorio, that uses the text of a source work."@en,
        "Una expresión de una obra musical no dramática, diferente de un oratorio, que usa el texto de la obra fuente."@es,
        "Expression d’une œuvre musicale non théâtrale, autre qu’un oratorio, qui utilise le texte de l’œuvre source."@fr ;
    rdakit:toolkitLabel "set to music as (expression)"@en,
        "hecha para música como (expresión)"@es,
        "mis en musique comme (expression)"@fr ;
    reg:hasSubproperty <http://rdaregistry.info/Elements/e/object/P20087> ;
    reg:hasUnconstrained <http://rdaregistry.info/Elements/u/P60121> ;
    reg:lexicalAlias <http://rdaregistry.info/Elements/e/setToMusicAsExpression.en> ;
    reg:name "setToMusicAsExpression"@en ;
    reg:status <http://metadataregistry.org/uri/RegStatus/1001> ;
    rdfs:domain <http://rdaregistry.info/Elements/c/C10006> ;
    rdfs:isDefinedBy <http://rdaregistry.info/Elements/e/> ;
    rdfs:subPropertyOf <http://rdaregistry.info/Elements/e/P20203> ;
    skos:definition "Relates an expression to an expression of a non-dramatic musical work, other than an oratorio, that uses the text of a source work."@en .

<http://rdaregistry.info/Elements/e/P20088> a rdf:Property ;
    rdfs:label "is adapted as novel (expression)"@en ;
    rdakit:instructionNumber "24.5" ;
    rdakit:toolkitDefinition "An expression of a novel adapted from a source expression."@en,
        "Una expresión de una novela adaptada de la expresión fuente."@es,
        "Expression d’un roman adapté de l’expression source."@fr ;
    rdakit:toolkitLabel "adapted as novel (expression)"@en,
        "adaptada como novela (expresión)"@es,
        "adapté en roman (expression)"@fr ;
    reg:hasSubproperty <http://rdaregistry.info/Elements/e/object/P20088> ;
    reg:hasUnconstrained <http://rdaregistry.info/Elements/u/P60138> ;
    reg:lexicalAlias <http://rdaregistry.info/Elements/e/adaptedAsNovelExpression.en> ;
    reg:name "adaptedAsNovelExpression"@en ;
    reg:status <http://metadataregistry.org/uri/RegStatus/1001> ;
    rdfs:domain <http://rdaregistry.info/Elements/c/C10006> ;
    rdfs:isDefinedBy <http://rdaregistry.info/Elements/e/> ;
    rdfs:subPropertyOf <http://rdaregistry.info/Elements/e/P20153> ;
    skos:definition "Relates an expression to an expression of a novel adapted from a source expression."@en .

<http://rdaregistry.info/Elements/e/P20089> a rdf:Property ;
    rdfs:label "is appendix to (expression)"@en ;
    rdakit:instructionNumber "24.5" ;
    rdakit:toolkitDefinition "An expression of a work whose content is augmented with content from an expression of another work."@en,
        "Una expresión de una obra que es aumentada por otra obra que consiste en material que no es esencial para la integridad del contenido, tal como una lista de referencias, tablas estadísticas, material explicativo; la obra adicional puede venir al final del contenido, o ser publicada separadamente"@es,
        "Expression d’une œuvre prédominante qui est augmentée par une autre œuvre qui consiste en informations qui ne sont pas essentielles à la complétude du contenu, telles qu’une liste de références, des tableaux statistiques et des indications explicatives ; l’œuvre augmentante peut soit figurer à la fin du contenu, soit être publiée séparément."@fr ;
    rdakit:toolkitLabel "appendix to (expression)"@en,
        "apéndice de (expresión)"@es,
        "annexe de (expression)"@fr ;
    reg:hasSubproperty <http://rdaregistry.info/Elements/e/object/P20089> ;
    reg:hasUnconstrained <http://rdaregistry.info/Elements/u/P60253> ;
    reg:lexicalAlias <http://rdaregistry.info/Elements/e/appendixToExpression.en> ;
    reg:name "appendixToExpression"@en ;
    reg:status <http://metadataregistry.org/uri/RegStatus/1001> ;
    rdfs:domain <http://rdaregistry.info/Elements/c/C10006> ;
    rdfs:isDefinedBy <http://rdaregistry.info/Elements/e/> ;
    rdfs:subPropertyOf <http://rdaregistry.info/Elements/e/P20192> ;
    skos:definition "Relates an expression to an expression of a work whose content is augmented with content from an expression of another work."@en ;
    skos:scopeNote "Includes lists of references, statistical tables, and explanatory matter that are not essential to the completeness of the content."@en .

<http://rdaregistry.info/Elements/e/P20090> a rdf:Property ;
    rdfs:label "is abstracted in (expression)"@en ;
    rdakit:instructionNumber "24.5" ;
    rdakit:toolkitDefinition "An expression of a work that is an abstracting and indexing service that abstracts the contents of a source expression."@en,
        "Una expresión de una obra (un servicio de indización y resúmenes) que resume el contenido de una expresión fuente."@es,
        "Expression d’une œuvre (service d’analyse et d’indexation) qui résume le contenu d’une expression source."@fr ;
    rdakit:toolkitLabel "abstracted in (expression)"@en,
        "resumida en (expresión)"@es,
        "résumé analytiquement dans (expression)"@fr ;
    reg:hasSubproperty <http://rdaregistry.info/Elements/e/object/P20090> ;
    reg:hasUnconstrained <http://rdaregistry.info/Elements/u/P60177> ;
    reg:lexicalAlias <http://rdaregistry.info/Elements/e/abstractedInExpression.en> ;
    reg:name "abstractedInExpression"@en ;
    reg:status <http://metadataregistry.org/uri/RegStatus/1001> ;
    rdfs:domain <http://rdaregistry.info/Elements/c/C10006> ;
    rdfs:isDefinedBy <http://rdaregistry.info/Elements/e/> ;
    rdfs:subPropertyOf <http://rdaregistry.info/Elements/e/P20203> ;
    skos:definition "Relates an expression to an expression of a work that is an abstracting and indexing service that abstracts the contents of a source expression."@en .

<http://rdaregistry.info/Elements/e/P20091> a rdf:Property ;
    rdfs:label "is indexed in (expression)"@en ;
    rdakit:instructionNumber "24.5" ;
    rdakit:toolkitDefinition "An expression of a work that is an abstracting and indexing service that indexes the contents of a source expression."@en,
        "Una expresión de una obra (un servicio de indización y resúmenes) que indiza el contenido de una expresión fuente."@es,
        "Expression d’une œuvre (service d’analyse et d’indexation) qui indexe le contenu d’une expression source."@fr ;
    rdakit:toolkitLabel "indexed in (expression)"@en,
        "indizada en (expresión)"@es,
        "indexé dans (expression)"@fr ;
    reg:hasSubproperty <http://rdaregistry.info/Elements/e/object/P20091> ;
    reg:hasUnconstrained <http://rdaregistry.info/Elements/u/P60178> ;
    reg:lexicalAlias <http://rdaregistry.info/Elements/e/indexedInExpression.en> ;
    reg:name "indexedInExpression"@en ;
    reg:status <http://metadataregistry.org/uri/RegStatus/1001> ;
    rdfs:domain <http://rdaregistry.info/Elements/c/C10006> ;
    rdfs:isDefinedBy <http://rdaregistry.info/Elements/e/> ;
    rdfs:subPropertyOf <http://rdaregistry.info/Elements/e/P20203> ;
    skos:definition "Relates an expression to an expression of a work that is an abstracting and indexing service that indexes the contents of a source expression."@en .

<http://rdaregistry.info/Elements/e/P20092> a rdf:Property ;
    rdfs:label "is adapted as choreography (expression)"@en ;
    rdakit:instructionNumber "24.5" ;
    rdakit:toolkitDefinition "An expression of a work consisting of movement based on a source work."@en,
        "Una expresión de una obra que consiste en movimiento (p. ej., danza) basada en la obra fuente."@es,
        "Expression d’une œuvre consistant en mouvement (par exemple, de la danse) basée sur l’œuvre source."@fr ;
    rdakit:toolkitLabel "adapted as choreography (expression)"@en,
        "adaptada como coreografía (expresión)"@es,
        "adapté en chorégraphie (expression)"@fr ;
    reg:hasSubproperty <http://rdaregistry.info/Elements/e/object/P20092> ;
    reg:hasUnconstrained <http://rdaregistry.info/Elements/u/P60180> ;
    reg:lexicalAlias <http://rdaregistry.info/Elements/e/adaptedAsChoreographyExpression.en> ;
    reg:name "adaptedAsChoreographyExpression"@en ;
    reg:status <http://metadataregistry.org/uri/RegStatus/1001> ;
    rdfs:domain <http://rdaregistry.info/Elements/c/C10006> ;
    rdfs:isDefinedBy <http://rdaregistry.info/Elements/e/> ;
    rdfs:subPropertyOf <http://rdaregistry.info/Elements/e/P20153> ;
    skos:definition "Relates an expression to an expression of a work consisting of movement based on a source work."@en .

<http://rdaregistry.info/Elements/e/P20093> a rdf:Property ;
    rdfs:label "is errata (expression)"@en ;
    rdakit:instructionNumber "24.5" ;
    rdakit:toolkitDefinition "An expression of a work consisting of errors discovered after the publication of a predominant work, with their corrections."@en,
        "Una expresión de una obra que consiste en los errores descubiertos después de la publicación de la obra principal, con sus correcciones."@es,
        "Expression d’une œuvre constituée des erreurs découvertes après la publication de l’œuvre prédominante, avec leurs corrections."@fr ;
    rdakit:toolkitLabel "errata (expression)"@en,
        "fe de erratas (expresión)"@es,
        "errata (expression)"@fr ;
    reg:hasSubproperty <http://rdaregistry.info/Elements/e/object/P20093> ;
    reg:hasUnconstrained <http://rdaregistry.info/Elements/u/P60181> ;
    reg:lexicalAlias <http://rdaregistry.info/Elements/e/errataExpression.en> ;
    reg:name "errataExpression"@en ;
    reg:status <http://metadataregistry.org/uri/RegStatus/1001> ;
    rdfs:domain <http://rdaregistry.info/Elements/c/C10006> ;
    rdfs:isDefinedBy <http://rdaregistry.info/Elements/e/> ;
    rdfs:subPropertyOf <http://rdaregistry.info/Elements/e/P20105> ;
    skos:definition "Relates an expression to an expression of a work consisting of errors discovered after publication of a predominant work, with their corrections."@en .

<http://rdaregistry.info/Elements/e/P20094> a rdf:Property ;
    rdfs:label "is illustrations (expression)"@en ;
    rdakit:instructionNumber "24.5" ;
    rdakit:toolkitDefinition "An expression of a work consisting of pictorial content designed to explain or decorate an augmented expression."@en,
        "Una expresión de una obra que consiste en contenido pictórico diseñado para explicar o decorar la entidad aumentada."@es,
        "Expression d’une œuvre consistant en contenu visuel destiné à expliquer ou à décorer l’expression augmentée."@fr ;
    rdakit:toolkitLabel "illustrations (expression)"@en,
        "ilustraciones (expresión)"@es,
        "illustrations (expression)"@fr ;
    reg:hasSubproperty <http://rdaregistry.info/Elements/e/object/P20094> ;
    reg:hasUnconstrained <http://rdaregistry.info/Elements/u/P60182> ;
    reg:lexicalAlias <http://rdaregistry.info/Elements/e/illustrationsExpression.en> ;
    reg:name "illustrationsExpression"@en ;
    reg:status <http://metadataregistry.org/uri/RegStatus/1001> ;
    rdfs:domain <http://rdaregistry.info/Elements/c/C10006> ;
    rdfs:isDefinedBy <http://rdaregistry.info/Elements/e/> ;
    rdfs:subPropertyOf <http://rdaregistry.info/Elements/e/P20105> ;
    skos:definition "Relates an expression to an expression of a work consisting of pictorial content designed to explain or decorate an augmented expression."@en .

<http://rdaregistry.info/Elements/e/P20095> a rdf:Property ;
    rdfs:label "is adapted as motion picture screenplay (expression)"@en ;
    rdakit:instructionNumber "24.5" ;
    rdakit:toolkitDefinition "An expression of a work consisting of a screenplay for a motion picture, based on a source work."@en,
        "Una expresión de una obra que consiste en el guión para una película cinematográfica, basado en la obra fuente."@es,
        "Expression d’une œuvre consistant en le scénario pour un film, basée sur l’œuvre source."@fr ;
    rdakit:toolkitLabel "adapted as motion picture screenplay (expression)"@en,
        "adaptada como guión cinematográfico (expresión)"@es,
        "adapté en scénario de film (expression)"@fr ;
    reg:hasSubproperty <http://rdaregistry.info/Elements/e/object/P20095> ;
    reg:hasUnconstrained <http://rdaregistry.info/Elements/u/P60184> ;
    reg:lexicalAlias <http://rdaregistry.info/Elements/e/adaptedAsMotionPictureScreenplayExpression.en> ;
    reg:name "adaptedAsMotionPictureScreenplayExpression"@en ;
    reg:status <http://metadataregistry.org/uri/RegStatus/1001> ;
    rdfs:domain <http://rdaregistry.info/Elements/c/C10006> ;
    rdfs:isDefinedBy <http://rdaregistry.info/Elements/e/> ;
    rdfs:subPropertyOf <http://rdaregistry.info/Elements/e/P20096> ;
    skos:definition "Relates an expression to an expression of a work consisting of a screenplay for a motion picture, based on a source work."@en .

<http://rdaregistry.info/Elements/e/P20097> a rdf:Property ;
    rdfs:label "is adapted as television screenplay (expression)"@en ;
    rdakit:instructionNumber "24.5" ;
    rdakit:toolkitDefinition "An expression of a work consisting of a screenplay for a television program, based on a source work."@en,
        "Una expresión de una obra que consiste en el guión para un programa de televisión, basado en la obra fuente."@es,
        "Expression d’une œuvre consistant en le scénario pour une émission de télévision, basée sur l’œuvre source."@fr ;
    rdakit:toolkitLabel "adapted as television screenplay (expression)"@en,
        "adaptada como guión para televisión (expresión)"@es,
        "adapté en scénario de télévision (expression)"@fr ;
    reg:hasSubproperty <http://rdaregistry.info/Elements/e/object/P20097> ;
    reg:hasUnconstrained <http://rdaregistry.info/Elements/u/P60186> ;
    reg:lexicalAlias <http://rdaregistry.info/Elements/e/adaptedAsTelevisionScreenplayExpression.en> ;
    reg:name "adaptedAsTelevisionScreenplayExpression"@en ;
    reg:status <http://metadataregistry.org/uri/RegStatus/1001> ;
    rdfs:domain <http://rdaregistry.info/Elements/c/C10006> ;
    rdfs:isDefinedBy <http://rdaregistry.info/Elements/e/> ;
    rdfs:subPropertyOf <http://rdaregistry.info/Elements/e/P20096> ;
    skos:definition "Relates an expression to an expression of a work consisting of a screenplay for a television program, based on a source work."@en .

<http://rdaregistry.info/Elements/e/P20098> a rdf:Property ;
    rdfs:label "is adapted as video screenplay (expression)"@en ;
    rdakit:instructionNumber "24.5" ;
    rdakit:toolkitDefinition "An expression of a work consisting of a screenplay for a video, based on a source work."@en,
        "Una expresión de una obra que consiste en el guión para un video, basado en la obra fuente."@es,
        "Expression d’une œuvre consistant en le scénario pour une vidéo, basée sur l’œuvre source."@fr ;
    rdakit:toolkitLabel "adapted as video screenplay (expression)"@en,
        "adaptada como guión para video (expresión)"@es,
        "adapté en scénario de vidéo (expression)"@fr ;
    reg:hasSubproperty <http://rdaregistry.info/Elements/e/object/P20098> ;
    reg:hasUnconstrained <http://rdaregistry.info/Elements/u/P60187> ;
    reg:lexicalAlias <http://rdaregistry.info/Elements/e/adaptedAsVideoScreenplayExpression.en> ;
    reg:name "adaptedAsVideoScreenplayExpression"@en ;
    reg:status <http://metadataregistry.org/uri/RegStatus/1001> ;
    rdfs:domain <http://rdaregistry.info/Elements/c/C10006> ;
    rdfs:isDefinedBy <http://rdaregistry.info/Elements/e/> ;
    rdfs:subPropertyOf <http://rdaregistry.info/Elements/e/P20096> ;
    skos:definition "Relates an expression to an expression of a work consisting of a screenplay for a video, based on a source work."@en .

<http://rdaregistry.info/Elements/e/P20099> a rdf:Property ;
    rdfs:label "is adapted as radio script (expression)"@en ;
    rdakit:instructionNumber "24.5" ;
    rdakit:toolkitDefinition "An expression of a work consisting of a script for a radio program, based on a source work."@en,
        "Una expresión de una obra que consiste en el guión de un programa de radio, basado en la obra fuente."@es,
        "Expression d’une œuvre consistant en le script d’une émission de radio, basée sur l’œuvre source."@fr ;
    rdakit:toolkitLabel "adapted as radio script (expression)"@en,
        "adaptada como guión radiofónico (expresión)"@es,
        "adapté en script radiophonique (expression)"@fr ;
    reg:hasSubproperty <http://rdaregistry.info/Elements/e/object/P20099> ;
    reg:hasUnconstrained <http://rdaregistry.info/Elements/u/P60188> ;
    reg:lexicalAlias <http://rdaregistry.info/Elements/e/adaptedAsRadioScriptExpression.en> ;
    reg:name "adaptedAsRadioScriptExpression"@en ;
    reg:status <http://metadataregistry.org/uri/RegStatus/1001> ;
    rdfs:domain <http://rdaregistry.info/Elements/c/C10006> ;
    rdfs:isDefinedBy <http://rdaregistry.info/Elements/e/> ;
    rdfs:subPropertyOf <http://rdaregistry.info/Elements/e/P20153> ;
    skos:definition "Relates an expression to an expression of a work consisting of a script for a radio program, based on a source work."@en .

<http://rdaregistry.info/Elements/e/P20101> a rdf:Property ;
    rdfs:label "is continued in part by (expression)"@en ;
    rdakit:instructionNumber "24.5" ;
    rdakit:toolkitDefinition "An expression of a work part of whose content separated from an earlier expression to form a new expression."@en,
        "Una expresión de una obra parte de cuyo contenido se separó de una expresión anterior para formar una nueva expresión."@es,
        "Expression d’une œuvre dont une partie du contenu a été détachée d’une expression antérieure pour former une nouvelle expression."@fr ;
    rdakit:toolkitLabel "continued in part by (expression)"@en,
        "continuada en parte por (expresión)"@es,
        "continué en partie par (expression)"@fr ;
    reg:hasSubproperty <http://rdaregistry.info/Elements/e/object/P20101> ;
    reg:hasUnconstrained <http://rdaregistry.info/Elements/u/P60199> ;
    reg:lexicalAlias <http://rdaregistry.info/Elements/e/continuedInPartByExpression.en> ;
    reg:name "continuedInPartByExpression"@en ;
    reg:status <http://metadataregistry.org/uri/RegStatus/1001> ;
    rdfs:domain <http://rdaregistry.info/Elements/c/C10006> ;
    rdfs:isDefinedBy <http://rdaregistry.info/Elements/e/> ;
    rdfs:subPropertyOf <http://rdaregistry.info/Elements/e/P20169> ;
    skos:definition "Relates an expression to an expression of a work part of whose content separated from an earlier expression to form a new expression."@en ;
    skos:scopeNote "This relationship applies generally to serials."@en .

<http://rdaregistry.info/Elements/e/P20103> a rdf:Property ;
    rdfs:label "is incidental music for (expression)"@en ;
    rdakit:instructionNumber "24.5" ;
    rdakit:toolkitDefinition "An expression of a work such as a play or other spoken work for the stage that uses a musical work as incidental music."@en,
        "Una expresión de una obra tal como una obra de teatro u otra obra hablada para escena que usa la obra musical como música incidental."@es,
        "Expression d’une œuvre telle qu’une pièce de théâtre ou une autre œuvre parlée pour la scène qui utilise l’œuvre musicale comme musique de scène."@fr ;
    rdakit:toolkitLabel "incidental music for (expression)"@en,
        "música incidental de (expresión)"@es,
        "musique de scène pour (expression)"@fr ;
    reg:hasSubproperty <http://rdaregistry.info/Elements/e/object/P20103> ;
    reg:hasUnconstrained <http://rdaregistry.info/Elements/u/P60202> ;
    reg:lexicalAlias <http://rdaregistry.info/Elements/e/incidentalMusicForExpression.en> ;
    reg:name "incidentalMusicForExpression"@en ;
    reg:status <http://metadataregistry.org/uri/RegStatus/1001> ;
    rdfs:domain <http://rdaregistry.info/Elements/c/C10006> ;
    rdfs:isDefinedBy <http://rdaregistry.info/Elements/e/> ;
    rdfs:subPropertyOf <http://rdaregistry.info/Elements/e/P20244> ;
    skos:definition "Relates an expression to an expression of a work such as a play or other spoken work for the stage that uses a musical work as incidental music."@en .

<http://rdaregistry.info/Elements/e/P20104> a rdf:Property ;
    rdfs:label "is abstracted as (expression)"@en ;
    rdakit:instructionNumber "24.5" ;
    rdakit:toolkitDefinition "An expression of a work that abbreviates a source expression in a brief, objective manner."@en,
        "Una expresión de una obra que abrevia la expresión fuente en una forma breve y objetiva."@es,
        "Expression d’une œuvre qui abrège l’expression source d’une manière brève et objective."@fr ;
    rdakit:toolkitLabel "abstracted as (expression)"@en,
        "resumida como (expresión)"@es,
        "résumé analytiquement comme (expression)"@fr ;
    reg:hasSubproperty <http://rdaregistry.info/Elements/e/object/P20104> ;
    reg:hasUnconstrained <http://rdaregistry.info/Elements/u/P60203> ;
    reg:lexicalAlias <http://rdaregistry.info/Elements/e/abstractedAsExpression.en> ;
    reg:name "abstractedAsExpression"@en ;
    reg:status <http://metadataregistry.org/uri/RegStatus/1001> ;
    rdfs:domain <http://rdaregistry.info/Elements/c/C10006> ;
    rdfs:isDefinedBy <http://rdaregistry.info/Elements/e/> ;
    rdfs:subPropertyOf <http://rdaregistry.info/Elements/e/P20203> ;
    skos:definition "Relates an expression to an expression of a work that abbreviates a source expression in a brief, objective manner."@en .

<http://rdaregistry.info/Elements/e/P20106> a rdf:Property ;
    rdfs:label "is summarized as (expression)"@en ;
    rdakit:instructionNumber "24.5" ;
    rdakit:toolkitDefinition "An expression of a work that consists of a brief recapitulation of the content of a source expression."@en,
        "Una expresión de una obra que consiste en una recapitulación breve del contenido de la expresión fuente."@es,
        "Expression d’une œuvre qui consiste en une brève récapitulation du contenu de l’expression source."@fr ;
    rdakit:toolkitLabel "summarized as (expression)"@en,
        "sumarizada como (expresión)"@es,
        "résumé comme (expression)"@fr ;
    reg:hasSubproperty <http://rdaregistry.info/Elements/e/object/P20106> ;
    reg:hasUnconstrained <http://rdaregistry.info/Elements/u/P60205> ;
    reg:lexicalAlias <http://rdaregistry.info/Elements/e/summarizedAsExpression.en> ;
    reg:name "summarizedAsExpression"@en ;
    reg:status <http://metadataregistry.org/uri/RegStatus/1001> ;
    rdfs:domain <http://rdaregistry.info/Elements/c/C10006> ;
    rdfs:isDefinedBy <http://rdaregistry.info/Elements/e/> ;
    rdfs:subPropertyOf <http://rdaregistry.info/Elements/e/P20203> ;
    skos:definition "Relates an expression to an expression of a work that consists of a brief recapitulation of the content of a source expression."@en .

<http://rdaregistry.info/Elements/e/P20107> a rdf:Property ;
    rdfs:label "is catalogue (expression)"@en ;
    rdakit:instructionNumber "24.5" ;
    rdakit:toolkitDefinition "An expression of a work that consists of a complete enumeration of items arranged systematically."@en,
        "Una expresión de una obra que consiste en una enumeración completa de ítems ordenados sistemáticamente."@es,
        "Expression d’une œuvre qui consiste en une énumération complète des items classés systématiquement."@fr ;
    rdakit:toolkitLabel "catalogue (expression)"@en,
        "catálogo (expresión)"@es,
        "catalogue (expression)"@fr ;
    reg:hasSubproperty <http://rdaregistry.info/Elements/e/object/P20107> ;
    reg:hasUnconstrained <http://rdaregistry.info/Elements/u/P60206> ;
    reg:lexicalAlias <http://rdaregistry.info/Elements/e/catalogueExpression.en> ;
    reg:name "catalogueExpression"@en ;
    reg:status <http://metadataregistry.org/uri/RegStatus/1001> ;
    rdfs:domain <http://rdaregistry.info/Elements/c/C10006> ;
    rdfs:isDefinedBy <http://rdaregistry.info/Elements/e/> ;
    rdfs:subPropertyOf <http://rdaregistry.info/Elements/e/P20105> ;
    skos:definition "Relates an expression to an expression of a work that consists of a complete enumeration of items arranged systematically."@en .

<http://rdaregistry.info/Elements/e/P20108> a rdf:Property ;
    rdfs:label "is concordance (expression)"@en ;
    rdakit:instructionNumber "24.5" ;
    rdakit:toolkitDefinition "An expression of a work that consists of an index of all the words in a predominant expression."@en,
        "Una expresión de una obra que consiste en un índice de todas las palabras en la expresión principal."@es,
        "Expression d’une œuvre qui consiste en un index de tous les mots de l’expression prédominante."@fr ;
    rdakit:toolkitLabel "concordance (expression)"@en,
        "concordancia (expresión)"@es,
        "concordance (expression)"@fr ;
    reg:hasSubproperty <http://rdaregistry.info/Elements/e/object/P20108> ;
    reg:hasUnconstrained <http://rdaregistry.info/Elements/u/P60208> ;
    reg:lexicalAlias <http://rdaregistry.info/Elements/e/concordanceExpression.en> ;
    reg:name "concordanceExpression"@en ;
    reg:status <http://metadataregistry.org/uri/RegStatus/1001> ;
    rdfs:domain <http://rdaregistry.info/Elements/c/C10006> ;
    rdfs:isDefinedBy <http://rdaregistry.info/Elements/e/> ;
    rdfs:subPropertyOf <http://rdaregistry.info/Elements/e/P20105> ;
    skos:definition "Relates an expression to an expression of a work that consists of an index of all the words in a predominant expression."@en .

<http://rdaregistry.info/Elements/e/P20109> a rdf:Property ;
    rdfs:label "is addenda (expression)"@en ;
    rdakit:instructionNumber "24.5" ;
    rdakit:toolkitDefinition "An expression of a work consisting of brief content that is essential for the completeness of an expression of another work."@en,
        "Una expresión de una obra que consiste en material adicional breve, menos extenso que un suplemento, pero esencial para la integridad del texto de la obra principal; generalmente se añade al final del contenido, pero algunas veces se publica separadamente."@es,
        "Expression d’une œuvre qui consiste en brèves informations additionnelles, moins étendues qu’un supplément, mais essentielles à la complétude du texte de l’œuvre prédominante ; ces informations sont généralement ajoutées à la fin du contenu, mais peuvent aussi parfois être publiées séparément."@fr ;
    rdakit:toolkitLabel "addenda (expression)"@en,
        "adenda (expresión)"@es,
        "addenda (expression)"@fr ;
    reg:hasSubproperty <http://rdaregistry.info/Elements/e/object/P20109> ;
    reg:hasUnconstrained <http://rdaregistry.info/Elements/u/P60209> ;
    reg:lexicalAlias <http://rdaregistry.info/Elements/e/addendaExpression.en> ;
    reg:name "addendaExpression"@en ;
    reg:status <http://metadataregistry.org/uri/RegStatus/1001> ;
    rdfs:domain <http://rdaregistry.info/Elements/c/C10006> ;
    rdfs:isDefinedBy <http://rdaregistry.info/Elements/e/> ;
    rdfs:subPropertyOf <http://rdaregistry.info/Elements/e/P20105> ;
    skos:definition "Relates an expression to an expression of a work consisting of brief content that is essential for the completeness of an expression of another work."@en .

<http://rdaregistry.info/Elements/e/P20110> a rdf:Property ;
    rdfs:label "is adapted as libretto (expression)"@en ;
    rdakit:instructionNumber "24.5" ;
    rdakit:toolkitDefinition "An expression of a work consisting of the text of an opera or other work for the musical stage, or an oratorio, based on a source work."@en,
        "Una expresión de una obra que consiste en el texto de una ópera u otra obra para representación musical, u oratorio, basada en la obra fuente."@es,
        "Expression d’une œuvre qui consiste en le texte d’un opéra ou d’une autre œuvre pour la scène musicale, ou bien d’un oratorio, basée sur l’œuvre source."@fr ;
    rdakit:toolkitLabel "adapted as libretto (expression)"@en,
        "adaptada como libreto (expresión)"@es,
        "adapté en livret (expression)"@fr ;
    reg:hasSubproperty <http://rdaregistry.info/Elements/e/object/P20110> ;
    reg:hasUnconstrained <http://rdaregistry.info/Elements/u/P60210> ;
    reg:lexicalAlias <http://rdaregistry.info/Elements/e/adaptedAsLibrettoExpression.en> ;
    reg:name "adaptedAsLibrettoExpression"@en ;
    reg:status <http://metadataregistry.org/uri/RegStatus/1001> ;
    rdfs:domain <http://rdaregistry.info/Elements/c/C10006> ;
    rdfs:isDefinedBy <http://rdaregistry.info/Elements/e/> ;
    rdfs:subPropertyOf <http://rdaregistry.info/Elements/e/P20153> ;
    skos:definition "Relates an expression to an expression of a work consisting of the text of an opera or other work for the musical stage, or an oratorio, based on a source work."@en .

<http://rdaregistry.info/Elements/e/P20111> a rdf:Property ;
    reg:status <http://metadataregistry.org/uri/RegStatus/1008> ;
    rdfs:isDefinedBy <http://rdaregistry.info/Elements/e/> ;
    rdfs:subPropertyOf <http://rdaregistry.info/Elements/e/P20202> .

<http://rdaregistry.info/Elements/e/P20112> a rdf:Property ;
    reg:status <http://metadataregistry.org/uri/RegStatus/1008> ;
    rdfs:isDefinedBy <http://rdaregistry.info/Elements/e/> ;
    rdfs:subPropertyOf <http://rdaregistry.info/Elements/e/P20202> .

<http://rdaregistry.info/Elements/e/P20113> a rdf:Property ;
    reg:status <http://metadataregistry.org/uri/RegStatus/1008> ;
    rdfs:isDefinedBy <http://rdaregistry.info/Elements/e/> ;
    rdfs:subPropertyOf <http://rdaregistry.info/Elements/e/P20202> .

<http://rdaregistry.info/Elements/e/P20115> a rdf:Property ;
    rdfs:label "is expanded as (expression)"@en ;
    rdakit:instructionNumber "24.5" ;
    rdakit:toolkitDefinition "An expression of a work that enlarges upon the content of the source work."@en,
        "Una expresión de una obra que extiende el contenido de la obra fuente."@es,
        "Expression d’une œuvre qui accroît le contenu de l’œuvre source."@fr ;
    rdakit:toolkitLabel "expanded as (expression)"@en,
        "ampliada como (expresión)"@es,
        "augmenté comme (expression)"@fr ;
    reg:hasSubproperty <http://rdaregistry.info/Elements/e/object/P20115> ;
    reg:hasUnconstrained <http://rdaregistry.info/Elements/u/P60216> ;
    reg:lexicalAlias <http://rdaregistry.info/Elements/e/expandedAsExpression.en> ;
    reg:name "expandedAsExpression"@en ;
    reg:status <http://metadataregistry.org/uri/RegStatus/1001> ;
    rdfs:domain <http://rdaregistry.info/Elements/c/C10006> ;
    rdfs:isDefinedBy <http://rdaregistry.info/Elements/e/> ;
    rdfs:subPropertyOf <http://rdaregistry.info/Elements/e/P20203> ;
    skos:definition "Relates an expression to an expression of a work that enlarges upon the content of a source work."@en .

<http://rdaregistry.info/Elements/e/P20116> a rdf:Property ;
    reg:status <http://metadataregistry.org/uri/RegStatus/1008> ;
    rdfs:isDefinedBy <http://rdaregistry.info/Elements/e/> ;
    rdfs:subPropertyOf <http://rdaregistry.info/Elements/e/P20202> .

<http://rdaregistry.info/Elements/e/P20117> a rdf:Property ;
    reg:status <http://metadataregistry.org/uri/RegStatus/1008> ;
    rdfs:isDefinedBy <http://rdaregistry.info/Elements/e/> ;
    rdfs:subPropertyOf <http://rdaregistry.info/Elements/e/P20202> .

<http://rdaregistry.info/Elements/e/P20118> a rdf:Property ;
    rdfs:label "is appendix (expression)"@en ;
    rdakit:instructionNumber "24.5" ;
    rdakit:toolkitDefinition "An expression of a work whose content augments an expression of another work."@en,
        "Una expresión de una obra que forma una parte adicional de otra obra y que no es esencial para la integridad del contenido, tal como una lista de referencias, tablas estadísticas y material explicativo; puede ser material que se presenta al final del contenido de la obra principal, o ser publicado separadamente."@es,
        "Expression d’une œuvre qui forme une partie augmentante d’une autre œuvre et qui n’est pas essentielle à la complétude du contenu, telle qu’une liste de références, des tableaux statistiques et des indications explicatives ; elle peut soit figurer à la fin du contenu de l’œuvre prédominante, soit être publiée séparément."@fr ;
    rdakit:toolkitLabel "appendix (expression)"@en,
        "apéndice (expresión)"@es,
        "annexe (expression)"@fr ;
    reg:hasSubproperty <http://rdaregistry.info/Elements/e/object/P20118> ;
    reg:hasUnconstrained <http://rdaregistry.info/Elements/u/P60221> ;
    reg:lexicalAlias <http://rdaregistry.info/Elements/e/appendixExpression.en> ;
    reg:name "appendixExpression"@en ;
    reg:status <http://metadataregistry.org/uri/RegStatus/1001> ;
    rdfs:domain <http://rdaregistry.info/Elements/c/C10006> ;
    rdfs:isDefinedBy <http://rdaregistry.info/Elements/e/> ;
    rdfs:subPropertyOf <http://rdaregistry.info/Elements/e/P20105> ;
    skos:definition "Relates an expression to an expression of a work whose content augments an expression of another work."@en ;
    skos:scopeNote "Includes lists of references, statistical tables, and explanatory matter that are not essential to the completeness of the content."@en .

<http://rdaregistry.info/Elements/e/P20119> a rdf:Property ;
    rdfs:label "is freely translated as (expression)"@en ;
    rdakit:instructionNumber "24.5" ;
    rdakit:toolkitDefinition "An expression of a work that is both an adaptation and a translation into another language of a source expression."@en,
        "Una expresión de una obra que traduce libremente el texto en otra lengua, preservando el espíritu del original, pero no sus detalles lingüísticos."@es,
        "Expression d’une œuvre qui traduit librement le texte dans une autre langue, de façon à préserver l’esprit de l’original, mais non ses particularités linguistiques."@fr ;
    rdakit:toolkitLabel "freely translated as (expression)"@en,
        "traducida libremente como (expresión)"@es,
        "librement traduit comme (expression)"@fr ;
    reg:hasSubproperty <http://rdaregistry.info/Elements/e/object/P20119> ;
    reg:hasUnconstrained <http://rdaregistry.info/Elements/u/P60189> ;
    reg:lexicalAlias <http://rdaregistry.info/Elements/e/freelyTranslatedAsExpression.en> ;
    reg:name "freelyTranslatedAsExpression"@en ;
    reg:status <http://metadataregistry.org/uri/RegStatus/1001> ;
    rdfs:domain <http://rdaregistry.info/Elements/c/C10006> ;
    rdfs:isDefinedBy <http://rdaregistry.info/Elements/e/> ;
    rdfs:subPropertyOf <http://rdaregistry.info/Elements/e/P20203> ;
    skos:definition "Relates an expression to an expression of a work that is both an adaptation and a translation into another language of a source expression."@en .

<http://rdaregistry.info/Elements/e/P20120> a rdf:Property ;
    rdfs:label "is guide (expression)"@en ;
    rdakit:instructionNumber "24.5" ;
    rdakit:toolkitDefinition "An expression of a work that guides a user through the use of a predominant work, using notes, learning and study aids, exercises, problems, questions and answers, instructor or student materials, etc."@en,
        "Una expresión de una obra que guía al usuario a través del uso de la obra principal, utilizando notas, ayudas de aprendizaje y estudio, ejercicios, problemas, preguntas y respuestas, materiales para el instructor o el estudiante, etc."@es,
        "Expression d’une œuvre qui guide un utilisateur à travers l’œuvre prédominante au moyen de notes, d’outils pédagogiques, d’exercices, de problèmes, de questions et réponses, de matériel didactique, etc."@fr ;
    rdakit:toolkitLabel "guide (expression)"@en,
        "guía (expresión)"@es,
        "guide (expression)"@fr ;
    reg:hasSubproperty <http://rdaregistry.info/Elements/e/object/P20120> ;
    reg:hasUnconstrained <http://rdaregistry.info/Elements/u/P60222> ;
    reg:lexicalAlias <http://rdaregistry.info/Elements/e/guideExpression.en> ;
    reg:name "guideExpression"@en ;
    reg:status <http://metadataregistry.org/uri/RegStatus/1001> ;
    rdfs:domain <http://rdaregistry.info/Elements/c/C10006> ;
    rdfs:isDefinedBy <http://rdaregistry.info/Elements/e/> ;
    rdfs:subPropertyOf <http://rdaregistry.info/Elements/e/P20105> ;
    skos:definition "Relates an expression to an expression of a work that guides a user through the use of a predominant work, using notes, learning and study aids, exercises, problems, questions and answers, instructor or student materials, etc."@en .

<http://rdaregistry.info/Elements/e/P20121> a rdf:Property ;
    rdfs:label "is abridgement of (expression)"@en ;
    rdakit:instructionNumber "24.5" ;
    rdakit:toolkitDefinition "An expression of a work that has been abridged, i.e., shortened without changing the general meaning or manner of presentation of a source work."@en,
        "Una expresión de una obra que fue abreviada, i.e., acortada sin cambiar el sentido general o la manera de presentación de la obra fuente."@es,
        "Expression d’une œuvre qui a été abrégée, c’est-à-dire raccourcie sans changer le sens général ou le mode de présentation de l’œuvre source."@fr ;
    rdakit:toolkitLabel "abridgement of (expression)"@en,
        "abreviada de (expresión)"@es,
        "abrégé de (expression)"@fr ;
    reg:hasSubproperty <http://rdaregistry.info/Elements/e/object/P20121> ;
    reg:hasUnconstrained <http://rdaregistry.info/Elements/u/P60223> ;
    reg:lexicalAlias <http://rdaregistry.info/Elements/e/abridgementOfExpression.en> ;
    reg:name "abridgementOfExpression"@en ;
    reg:status <http://metadataregistry.org/uri/RegStatus/1001> ;
    rdfs:domain <http://rdaregistry.info/Elements/c/C10006> ;
    rdfs:isDefinedBy <http://rdaregistry.info/Elements/e/> ;
    rdfs:subPropertyOf <http://rdaregistry.info/Elements/e/P20204> ;
    skos:definition "Relates an expression to an expression of a work that has been abridged, i.e., shortened without changing the general meaning or manner of presentation of a source work."@en .

<http://rdaregistry.info/Elements/e/P20122> a rdf:Property ;
    rdfs:label "is abstract of (expression)"@en ;
    rdakit:instructionNumber "24.5" ;
    rdakit:toolkitDefinition "An expression of a work that has been abstracted, i.e., abbreviated in a brief, objective manner."@en,
        "Una expresión de una obra que fue resumida, i.e., abreviada en una forma breve, objetiva."@es,
        "Expression d’une œuvre qui a été résumée analytiquement, c’est-à-dire abrégée d’une manière brève et objective."@fr ;
    rdakit:toolkitLabel "abstract of (expression)"@en,
        "resumen de (expresión)"@es,
        "résumé analytique de (expression)"@fr ;
    reg:hasSubproperty <http://rdaregistry.info/Elements/e/object/P20122> ;
    reg:hasUnconstrained <http://rdaregistry.info/Elements/u/P60224> ;
    reg:lexicalAlias <http://rdaregistry.info/Elements/e/abstractOfExpression.en> ;
    reg:name "abstractOfExpression"@en ;
    reg:status <http://metadataregistry.org/uri/RegStatus/1001> ;
    rdfs:domain <http://rdaregistry.info/Elements/c/C10006> ;
    rdfs:isDefinedBy <http://rdaregistry.info/Elements/e/> ;
    rdfs:subPropertyOf <http://rdaregistry.info/Elements/e/P20204> ;
    skos:definition "Relates an expression to an expression of a work that has been abstracted, i.e., abbreviated in a brief, objective manner."@en .

<http://rdaregistry.info/Elements/e/P20123> a rdf:Property ;
    rdfs:label "is dramatization of (expression)"@en ;
    rdakit:instructionNumber "24.5" ;
    rdakit:toolkitDefinition "An expression of a work that has been adapted as a drama."@en,
        "Una expresión de una obra que fue adaptada como drama."@es,
        "Expression d’une œuvre qui a été adaptée en pièce de théâtre."@fr ;
    rdakit:toolkitLabel "dramatization of (expression)"@en,
        "dramatización de (expresión)"@es,
        "adaptation au théâtre de (expression)"@fr ;
    reg:hasSubproperty <http://rdaregistry.info/Elements/e/object/P20123> ;
    reg:hasUnconstrained <http://rdaregistry.info/Elements/u/P60225> ;
    reg:lexicalAlias <http://rdaregistry.info/Elements/e/dramatizationOfExpression.en> ;
    reg:name "dramatizationOfExpression"@en ;
    reg:status <http://metadataregistry.org/uri/RegStatus/1001> ;
    rdfs:domain <http://rdaregistry.info/Elements/c/C10006> ;
    rdfs:isDefinedBy <http://rdaregistry.info/Elements/e/> ;
    rdfs:subPropertyOf <http://rdaregistry.info/Elements/e/P20152> ;
    skos:definition "Relates an expression to an expression of a work that has been adapted as a drama."@en .

<http://rdaregistry.info/Elements/e/P20124> a rdf:Property ;
    rdfs:label "is verse adaptation of (expression)"@en ;
    rdakit:instructionNumber "24.5" ;
    rdakit:toolkitDefinition "An expression of a work that has been adapted as a literary composition in verse form."@en,
        "Una expresión de una obra que fue adaptada como una composición literaria en forma de verso."@es,
        "Expression d’une œuvre qui a été adaptée sous forme de composition littéraire en vers."@fr ;
    rdakit:toolkitLabel "verse adaptation of (expression)"@en,
        "adaptación en verso de (expresión)"@es,
        "adaptation en vers de (expression)"@fr ;
    reg:hasSubproperty <http://rdaregistry.info/Elements/e/object/P20124> ;
    reg:hasUnconstrained <http://rdaregistry.info/Elements/u/P60226> ;
    reg:lexicalAlias <http://rdaregistry.info/Elements/e/verseAdaptationOfExpression.en> ;
    reg:name "verseAdaptationOfExpression"@en ;
    reg:status <http://metadataregistry.org/uri/RegStatus/1001> ;
    rdfs:domain <http://rdaregistry.info/Elements/c/C10006> ;
    rdfs:isDefinedBy <http://rdaregistry.info/Elements/e/> ;
    rdfs:subPropertyOf <http://rdaregistry.info/Elements/e/P20152> ;
    skos:definition "Relates an expression to an expression of a work that has been adapted as a literary composition in verse form."@en .

<http://rdaregistry.info/Elements/e/P20125> a rdf:Property ;
    rdfs:label "is motion picture adaptation of (expression)"@en ;
    rdakit:instructionNumber "24.5" ;
    rdakit:toolkitDefinition "An expression of a work that has been adapted as a motion picture."@en,
        "Una expresión de una obra que fue adaptada como película cinematográfica."@es,
        "Expression d’une œuvre qui a été adaptée en film."@fr ;
    rdakit:toolkitLabel "motion picture adaptation of (expression)"@en,
        "adaptación cinematográfica de (expresión)"@es,
        "adaptation au cinéma de (expression)"@fr ;
    reg:hasSubproperty <http://rdaregistry.info/Elements/e/object/P20125> ;
    reg:hasUnconstrained <http://rdaregistry.info/Elements/u/P60227> ;
    reg:lexicalAlias <http://rdaregistry.info/Elements/e/motionPictureAdaptationOfExpression.en> ;
    reg:name "motionPictureAdaptationOfExpression"@en ;
    reg:status <http://metadataregistry.org/uri/RegStatus/1001> ;
    rdfs:domain <http://rdaregistry.info/Elements/c/C10006> ;
    rdfs:isDefinedBy <http://rdaregistry.info/Elements/e/> ;
    rdfs:subPropertyOf <http://rdaregistry.info/Elements/e/P20152> ;
    skos:definition "Relates an expression to an expression of a work that has been adapted as a motion picture."@en .

<http://rdaregistry.info/Elements/e/P20126> a rdf:Property ;
    rdfs:label "is novelization of (expression)"@en ;
    rdakit:instructionNumber "24.5" ;
    rdakit:toolkitDefinition "An expression of a work that has been adapted as a novel."@en,
        "Una expresión de una obra que fue adaptada como novela."@es,
        "Expression d’une œuvre qui a été adaptée en roman."@fr ;
    rdakit:toolkitLabel "novelization of (expression)"@en,
        "novelización de (expresión)"@es,
        "novélisation de (expression)"@fr ;
    reg:hasSubproperty <http://rdaregistry.info/Elements/e/object/P20126> ;
    reg:hasUnconstrained <http://rdaregistry.info/Elements/u/P60228> ;
    reg:lexicalAlias <http://rdaregistry.info/Elements/e/novelizationOfExpression.en> ;
    reg:name "novelizationOfExpression"@en ;
    reg:status <http://metadataregistry.org/uri/RegStatus/1001> ;
    rdfs:domain <http://rdaregistry.info/Elements/c/C10006> ;
    rdfs:isDefinedBy <http://rdaregistry.info/Elements/e/> ;
    rdfs:subPropertyOf <http://rdaregistry.info/Elements/e/P20152> ;
    skos:definition "Relates an expression to an expression of a work that has been adapted as a novel."@en .

<http://rdaregistry.info/Elements/e/P20127> a rdf:Property ;
    rdfs:label "is radio adaptation of (expression)"@en ;
    rdakit:instructionNumber "24.5" ;
    rdakit:toolkitDefinition "An expression of a work that has been adapted as a radio program."@en,
        "Una expresión de una obra que fue adaptada como programa de radio."@es,
        "Expression d’une œuvre qui a été adaptée en émission de radio."@fr ;
    rdakit:toolkitLabel "radio adaptation of (expression)"@en,
        "adaptación para radio de (expresión)"@es,
        "adaptation pour la radio de (expression)"@fr ;
    reg:hasSubproperty <http://rdaregistry.info/Elements/e/object/P20127> ;
    reg:hasUnconstrained <http://rdaregistry.info/Elements/u/P60229> ;
    reg:lexicalAlias <http://rdaregistry.info/Elements/e/radioAdaptationOfExpression.en> ;
    reg:name "radioAdaptationOfExpression"@en ;
    reg:status <http://metadataregistry.org/uri/RegStatus/1001> ;
    rdfs:domain <http://rdaregistry.info/Elements/c/C10006> ;
    rdfs:isDefinedBy <http://rdaregistry.info/Elements/e/> ;
    rdfs:subPropertyOf <http://rdaregistry.info/Elements/e/P20152> ;
    skos:definition "Relates an expression to an expression of a work that has been adapted as a radio program."@en .

<http://rdaregistry.info/Elements/e/P20128> a rdf:Property ;
    rdfs:label "is television adaptation of (expression)"@en ;
    rdakit:instructionNumber "24.5" ;
    rdakit:toolkitDefinition "An expression of a work that has been adapted as a television program."@en,
        "Una expresión de una obra que fue adaptada como programa de televisión."@es,
        "Expression d’une œuvre qui a été adaptée en émission de télévision."@fr ;
    rdakit:toolkitLabel "television adaptation of (expression)"@en,
        "adaptación para televisión de (expresión)"@es,
        "adaptation pour la télévision de (expression)"@fr ;
    reg:hasSubproperty <http://rdaregistry.info/Elements/e/object/P20128> ;
    reg:hasUnconstrained <http://rdaregistry.info/Elements/u/P60230> ;
    reg:lexicalAlias <http://rdaregistry.info/Elements/e/televisionAdaptationOfExpression.en> ;
    reg:name "televisionAdaptationOfExpression"@en ;
    reg:status <http://metadataregistry.org/uri/RegStatus/1001> ;
    rdfs:domain <http://rdaregistry.info/Elements/c/C10006> ;
    rdfs:isDefinedBy <http://rdaregistry.info/Elements/e/> ;
    rdfs:subPropertyOf <http://rdaregistry.info/Elements/e/P20152> ;
    skos:definition "Relates an expression to an expression of a work that has been adapted as a television program."@en .

<http://rdaregistry.info/Elements/e/P20130> a rdf:Property ;
    rdfs:label "is motion picture screenplay based on (expression)"@en ;
    rdakit:instructionNumber "24.5" ;
    rdakit:toolkitDefinition "An expression of a work that has been adapted as a screenplay for a motion picture."@en,
        "Una expresión de una obra que fue adaptada como guión para una película cinematográfica, programa de televisión o vídeo."@es,
        "Expression d’une œuvre qui a été adaptée en scénario pour un film."@fr ;
    rdakit:toolkitLabel "motion picture screenplay based on (expression)"@en,
        "guión cinematográfico basado en (expresión)"@es,
        "scénario de film basé sur (expression)"@fr ;
    reg:hasSubproperty <http://rdaregistry.info/Elements/e/object/P20130> ;
    reg:hasUnconstrained <http://rdaregistry.info/Elements/u/P60232> ;
    reg:lexicalAlias <http://rdaregistry.info/Elements/e/motionPictureScreenplayBasedOnExpression.en> ;
    reg:name "motionPictureScreenplayBasedOnExpression"@en ;
    reg:status <http://metadataregistry.org/uri/RegStatus/1001> ;
    rdfs:domain <http://rdaregistry.info/Elements/c/C10006> ;
    rdfs:isDefinedBy <http://rdaregistry.info/Elements/e/> ;
    rdfs:subPropertyOf <http://rdaregistry.info/Elements/e/P20129> ;
    skos:definition "Relates an expression to an expression of a work that has been adapted as a screenplay for a motion picture."@en .

<http://rdaregistry.info/Elements/e/P20131> a rdf:Property ;
    rdfs:label "is television screenplay based on (expression)"@en ;
    rdakit:instructionNumber "24.5" ;
    rdakit:toolkitDefinition "An expression of a work that has been adapted as a screenplay for a television program."@en,
        "Una expresión de una obra que fue adaptada como guión para un programa de televisión."@es,
        "Expression d’une œuvre qui a été adaptée en scénario pour une émission de télévision."@fr ;
    rdakit:toolkitLabel "television screenplay based on (expression)"@en,
        "guión para televisión basado en (expresión)"@es,
        "scénario de télévision basé sur (expression)"@fr ;
    reg:hasSubproperty <http://rdaregistry.info/Elements/e/object/P20131> ;
    reg:hasUnconstrained <http://rdaregistry.info/Elements/u/P60233> ;
    reg:lexicalAlias <http://rdaregistry.info/Elements/e/televisionScreenplayBasedOnExpression.en> ;
    reg:name "televisionScreenplayBasedOnExpression"@en ;
    reg:status <http://metadataregistry.org/uri/RegStatus/1001> ;
    rdfs:domain <http://rdaregistry.info/Elements/c/C10006> ;
    rdfs:isDefinedBy <http://rdaregistry.info/Elements/e/> ;
    rdfs:subPropertyOf <http://rdaregistry.info/Elements/e/P20129> ;
    skos:definition "Relates an expression to an expression of a work that has been adapted as a screenplay for a television program."@en .

<http://rdaregistry.info/Elements/e/P20132> a rdf:Property ;
    rdfs:label "is video screenplay based on (expression)"@en ;
    rdakit:instructionNumber "24.5" ;
    rdakit:toolkitDefinition "An expression of a work that has been adapted as a screenplay for a video."@en,
        "Una expresión de una obra que fue adaptada como guión para un video."@es,
        "Expression d’une œuvre qui a été adaptée en scénario pour une vidéo."@fr ;
    rdakit:toolkitLabel "video screenplay based on (expression)"@en,
        "guión para video basado en (expresión)"@es,
        "scénario de vidéo basé sur (expression)"@fr ;
    reg:hasSubproperty <http://rdaregistry.info/Elements/e/object/P20132> ;
    reg:hasUnconstrained <http://rdaregistry.info/Elements/u/P60234> ;
    reg:lexicalAlias <http://rdaregistry.info/Elements/e/videoScreenplayBasedOnExpression.en> ;
    reg:name "videoScreenplayBasedOnExpression"@en ;
    reg:status <http://metadataregistry.org/uri/RegStatus/1001> ;
    rdfs:domain <http://rdaregistry.info/Elements/c/C10006> ;
    rdfs:isDefinedBy <http://rdaregistry.info/Elements/e/> ;
    rdfs:subPropertyOf <http://rdaregistry.info/Elements/e/P20129> ;
    skos:definition "Relates an expression to an expression of a work that has been adapted as a screenplay for a video."@en .

<http://rdaregistry.info/Elements/e/P20133> a rdf:Property ;
    rdfs:label "is radio script based on (expression)"@en ;
    rdakit:instructionNumber "24.5" ;
    rdakit:toolkitDefinition "An expression of a work that has been adapted as a script for a radio program."@en,
        "Una expresión de una obra que fue adaptada como el guión de un programa de radio."@es,
        "Expression d’une œuvre qui a été adaptée en script d’émission de radio."@fr ;
    rdakit:toolkitLabel "radio script based on (expression)"@en,
        "guión radiofónico basado en (expresión)"@es,
        "script radiophonique basé sur (expression)"@fr ;
    reg:hasSubproperty <http://rdaregistry.info/Elements/e/object/P20133> ;
    reg:hasUnconstrained <http://rdaregistry.info/Elements/u/P60235> ;
    reg:lexicalAlias <http://rdaregistry.info/Elements/e/radioScriptBasedOnExpression.en> ;
    reg:name "radioScriptBasedOnExpression"@en ;
    reg:status <http://metadataregistry.org/uri/RegStatus/1001> ;
    rdfs:domain <http://rdaregistry.info/Elements/c/C10006> ;
    rdfs:isDefinedBy <http://rdaregistry.info/Elements/e/> ;
    rdfs:subPropertyOf <http://rdaregistry.info/Elements/e/P20152> ;
    skos:definition "Relates an expression to an expression of a work that has been adapted as the script for a radio program."@en .

<http://rdaregistry.info/Elements/e/P20134> a rdf:Property ;
    rdfs:label "is video adaptation of (expression)"@en ;
    rdakit:instructionNumber "24.5" ;
    rdakit:toolkitDefinition "An expression of a work that has been adapted for video."@en,
        "Una expresión de una obra que fue adaptada para video."@es,
        "Expression d’une œuvre qui a été adaptée en vidéo."@fr ;
    rdakit:toolkitLabel "video adaptation of (expression)"@en,
        "adaptación para video de (expresión)"@es,
        "adaptation en vidéo de (expression)"@fr ;
    reg:hasSubproperty <http://rdaregistry.info/Elements/e/object/P20134> ;
    reg:hasUnconstrained <http://rdaregistry.info/Elements/u/P60236> ;
    reg:lexicalAlias <http://rdaregistry.info/Elements/e/videoAdaptationOfExpression.en> ;
    reg:name "videoAdaptationOfExpression"@en ;
    reg:status <http://metadataregistry.org/uri/RegStatus/1001> ;
    rdfs:domain <http://rdaregistry.info/Elements/c/C10006> ;
    rdfs:isDefinedBy <http://rdaregistry.info/Elements/e/> ;
    rdfs:subPropertyOf <http://rdaregistry.info/Elements/e/P20152> ;
    skos:definition "Relates an expression to an expression of a work that has been adapted for video."@en .

<http://rdaregistry.info/Elements/e/P20135> a rdf:Property ;
    rdfs:label "is digest of (expression)"@en ;
    rdakit:instructionNumber "24.5" ;
    rdakit:toolkitDefinition "An expression of a work that has been digested, i.e., systematically and comprehensively condensed."@en,
        "Una expresión de una obra que ha sido resumida, i.e., condensada sistemática e integralmente."@es,
        "Expression d’une œuvre qui a été condensée, c’est-à-dire abrégée de manière systématique et complète."@fr ;
    rdakit:toolkitLabel "digest of (expression)"@en,
        "compendio de (expresión)"@es,
        "condensé de (expression)"@fr ;
    reg:hasSubproperty <http://rdaregistry.info/Elements/e/object/P20135> ;
    reg:hasUnconstrained <http://rdaregistry.info/Elements/u/P60238> ;
    reg:lexicalAlias <http://rdaregistry.info/Elements/e/digestOfExpression.en> ;
    reg:name "digestOfExpression"@en ;
    reg:status <http://metadataregistry.org/uri/RegStatus/1001> ;
    rdfs:domain <http://rdaregistry.info/Elements/c/C10006> ;
    rdfs:isDefinedBy <http://rdaregistry.info/Elements/e/> ;
    rdfs:subPropertyOf <http://rdaregistry.info/Elements/e/P20204> ;
    skos:definition "Relates an expression to an expression of a work that has been digested, i.e., systematically and comprehensively condensed."@en .

<http://rdaregistry.info/Elements/e/P20136> a rdf:Property ;
    reg:status <http://metadataregistry.org/uri/RegStatus/1008> ;
    rdfs:isDefinedBy <http://rdaregistry.info/Elements/e/> ;
    rdfs:subPropertyOf <http://rdaregistry.info/Elements/e/P20072> .

<http://rdaregistry.info/Elements/e/P20137> a rdf:Property ;
    rdfs:label "is absorption of (expression)"@en ;
    rdakit:instructionNumber "24.5" ;
    rdakit:toolkitDefinition "An expression of a work that has been incorporated into another expression."@en,
        "Una expresión de una obra que se ha incorporado en otra expresión."@es,
        "Expression d’une œuvre qui a été intégrée dans une autre expression."@fr ;
    rdakit:toolkitLabel "absorption of (expression)"@en,
        "absorción de (expresión)"@es,
        "absorption de (expression)"@fr ;
    reg:hasSubproperty <http://rdaregistry.info/Elements/e/object/P20137> ;
    reg:hasUnconstrained <http://rdaregistry.info/Elements/u/P60574> ;
    reg:lexicalAlias <http://rdaregistry.info/Elements/e/absorptionOfExpression.en> ;
    reg:name "absorptionOfExpression"@en ;
    reg:status <http://metadataregistry.org/uri/RegStatus/1001> ;
    rdfs:domain <http://rdaregistry.info/Elements/c/C10006> ;
    rdfs:isDefinedBy <http://rdaregistry.info/Elements/e/> ;
    rdfs:subPropertyOf <http://rdaregistry.info/Elements/e/P20154> ;
    skos:definition "Relates an expression to an expression of a work that has been incorporated into another expression."@en .

<http://rdaregistry.info/Elements/e/P20138> a rdf:Property ;
    rdfs:label "is absorption in part of (expression)"@en ;
    rdakit:instructionNumber "24.5" ;
    rdakit:toolkitDefinition "An expression of a work that has been partially incorporated into another expression."@en,
        "Una expresión de una obra que se ha incorporado parcialmente en otra expresión."@es,
        "Expression d’une œuvre qui a été partiellement intégrée dans une autre expression."@fr ;
    rdakit:toolkitLabel "absorption in part of (expression)"@en,
        "absorción en parte de (expresión)"@es,
        "absorption partielle de (expression)"@fr ;
    reg:hasSubproperty <http://rdaregistry.info/Elements/e/object/P20138> ;
    reg:hasUnconstrained <http://rdaregistry.info/Elements/u/P60575> ;
    reg:lexicalAlias <http://rdaregistry.info/Elements/e/absorptionInPartOfExpression.en> ;
    reg:name "absorptionInPartOfExpression"@en ;
    reg:status <http://metadataregistry.org/uri/RegStatus/1001> ;
    rdfs:domain <http://rdaregistry.info/Elements/c/C10006> ;
    rdfs:isDefinedBy <http://rdaregistry.info/Elements/e/> ;
    rdfs:subPropertyOf <http://rdaregistry.info/Elements/e/P20154> ;
    skos:definition "Relates an expression to an expression of a work that has been partially incorporated into another expression."@en .

<http://rdaregistry.info/Elements/e/P20139> a rdf:Property ;
    rdfs:label "is arrangement of"@en ;
    rdakit:instructionNumber "24.5" ;
    rdakit:toolkitDefinition "An expression of a musical work that has been rewritten for a medium of performance different from that for which the work was originally intended."@en,
        "Una expresión de una obra musical que fue reescrita para un medio de interpretación diferente de aquel para la que fue originalmente prevista."@es,
        "Expression d’une œuvre qui a été réécrite pour une distribution d’exécution différente de celle à laquelle l’œuvre était destinée à l’origine."@fr ;
    rdakit:toolkitLabel "arrangement of"@en,
        "arreglo de"@es,
        "arrangement de"@fr ;
    reg:hasSubproperty <http://rdaregistry.info/Elements/e/object/P20139> ;
    reg:hasUnconstrained <http://rdaregistry.info/Elements/u/P60242> ;
    reg:lexicalAlias <http://rdaregistry.info/Elements/e/arrangementOf.en> ;
    reg:name "arrangementOf"@en ;
    reg:status <http://metadataregistry.org/uri/RegStatus/1001> ;
    rdfs:domain <http://rdaregistry.info/Elements/c/C10006> ;
    rdfs:isDefinedBy <http://rdaregistry.info/Elements/e/> ;
    rdfs:subPropertyOf <http://rdaregistry.info/Elements/e/P20204> ;
    skos:definition "Relates an expression to an expression of a musical work that has been rewritten for a medium of performance different from that for which the work was originally intended."@en .

<http://rdaregistry.info/Elements/e/P20140> a rdf:Property ;
    rdfs:label "is free translation of (expression)"@en ;
    rdakit:instructionNumber "24.5" ;
    rdakit:toolkitDefinition "An expression of a work that has been adapted and translated into another language."@en,
        "Una expresión de una obra que fue traducida libremente, preservando el espíritu del original, pero no sus detalles lingüísticos."@es,
        "Expression d’une œuvre qui a été librement traduite en préservant l’esprit de l’original, mais non ses particularités linguistiques."@fr ;
    rdakit:toolkitLabel "free translation of (expression)"@en,
        "traducción libre de (expresión)"@es,
        "traduction libre de (expression)"@fr ;
    reg:hasSubproperty <http://rdaregistry.info/Elements/e/object/P20140> ;
    reg:hasUnconstrained <http://rdaregistry.info/Elements/u/P60243> ;
    reg:lexicalAlias <http://rdaregistry.info/Elements/e/freeTranslationOfExpression.en> ;
    reg:name "freeTranslationOfExpression"@en ;
    reg:status <http://metadataregistry.org/uri/RegStatus/1001> ;
    rdfs:domain <http://rdaregistry.info/Elements/c/C10006> ;
    rdfs:isDefinedBy <http://rdaregistry.info/Elements/e/> ;
    rdfs:subPropertyOf <http://rdaregistry.info/Elements/e/P20204> ;
    skos:definition "Relates an expression to an expression of a work that has been adapted and translated into another language."@en .

<http://rdaregistry.info/Elements/e/P20142> a rdf:Property ;
    rdfs:label "is parodied as (expression)"@en ;
    rdakit:instructionNumber "24.5" ;
    rdakit:toolkitDefinition "An expression of a work that imitates the style or content of a source work for comic effect."@en,
        "Una expresión de una obra que imita el estilo o contenido de la obra fuente para crear un efecto cómico."@es,
        "Expression d’une œuvre qui imite le style ou le contenu de l’œuvre source dans le but de produire un effet comique."@fr ;
    rdakit:toolkitLabel "parodied as (expression)"@en,
        "parodiada como (expresión)"@es,
        "parodié comme (expression)"@fr ;
    reg:hasSubproperty <http://rdaregistry.info/Elements/e/object/P20142> ;
    reg:hasUnconstrained <http://rdaregistry.info/Elements/u/P60246> ;
    reg:lexicalAlias <http://rdaregistry.info/Elements/e/parodiedAsExpression.en> ;
    reg:name "parodiedAsExpression"@en ;
    reg:status <http://metadataregistry.org/uri/RegStatus/1001> ;
    rdfs:domain <http://rdaregistry.info/Elements/c/C10006> ;
    rdfs:isDefinedBy <http://rdaregistry.info/Elements/e/> ;
    rdfs:subPropertyOf <http://rdaregistry.info/Elements/e/P20114> ;
    skos:definition "Relates an expression to an expression of a work that imitates the style or content of a source work for comic effect."@en .

<http://rdaregistry.info/Elements/e/P20143> a rdf:Property ;
    rdfs:label "is absorbed by (expression)"@en ;
    rdakit:instructionNumber "24.5" ;
    rdakit:toolkitDefinition "An expression of a work that incorporates another expression."@en,
        "Una expresión de una obra que incorpora otra expresión."@es,
        "Expression d’une œuvre qui intègre une autre expression."@fr ;
    rdakit:toolkitLabel "absorbed by (expression)"@en,
        "absorbida por (expresión)"@es,
        "absorbé par (expression)"@fr ;
    reg:hasSubproperty <http://rdaregistry.info/Elements/e/object/P20143> ;
    reg:hasUnconstrained <http://rdaregistry.info/Elements/u/P60247> ;
    reg:lexicalAlias <http://rdaregistry.info/Elements/e/absorbedByExpression.en> ;
    reg:name "absorbedByExpression"@en ;
    reg:status <http://metadataregistry.org/uri/RegStatus/1001> ;
    rdfs:domain <http://rdaregistry.info/Elements/c/C10006> ;
    rdfs:isDefinedBy <http://rdaregistry.info/Elements/e/> ;
    rdfs:subPropertyOf <http://rdaregistry.info/Elements/e/P20169> ;
    skos:definition "Relates an expression to an expression of a work that incorporates another expression."@en .

<http://rdaregistry.info/Elements/e/P20144> a rdf:Property ;
    rdfs:label "is absorbed in part by (expression)"@en ;
    rdakit:instructionNumber "24.5" ;
    rdakit:toolkitDefinition "An expression of a work that incorporates part of the content of another expression."@en,
        "Una expresión de una obra que incorpora parte del contenido de otra expresión."@es,
        "Expression d’une œuvre qui intègre une partie du contenu d’une autre expression."@fr ;
    rdakit:toolkitLabel "absorbed in part by (expression)"@en,
        "absorbida en parte por (expresión)"@es,
        "absorbé en partie par (expression)"@fr ;
    reg:hasSubproperty <http://rdaregistry.info/Elements/e/object/P20144> ;
    reg:hasUnconstrained <http://rdaregistry.info/Elements/u/P60248> ;
    reg:lexicalAlias <http://rdaregistry.info/Elements/e/absorbedInPartByExpression.en> ;
    reg:name "absorbedInPartByExpression"@en ;
    reg:status <http://metadataregistry.org/uri/RegStatus/1001> ;
    rdfs:domain <http://rdaregistry.info/Elements/c/C10006> ;
    rdfs:isDefinedBy <http://rdaregistry.info/Elements/e/> ;
    rdfs:subPropertyOf <http://rdaregistry.info/Elements/e/P20169> ;
    skos:definition "Relates an expression to an expression of a work that incorporates part of the content of another expression."@en .

<http://rdaregistry.info/Elements/e/P20145> a rdf:Property ;
    rdfs:label "is container of (expression)"@en ;
    rdakit:instructionNumber "24.5" ;
    rdakit:toolkitDefinition "An expression of a work that is a discrete component of a larger expression."@en,
        "Una expresión de una obra que es un componente separado de una expresión mayor."@es,
        "Expression d’une œuvre qui est une composante distincte d’une expression plus vaste."@fr ;
    rdakit:toolkitLabel "container of (expression)"@en,
        "contiene (expresión)"@es,
        "conteneur de (expression)"@fr ;
    reg:hasSubproperty <http://rdaregistry.info/Elements/e/object/P20145> ;
    reg:hasUnconstrained <http://rdaregistry.info/Elements/u/P60249> ;
    reg:lexicalAlias <http://rdaregistry.info/Elements/e/containerOfExpression.en> ;
    reg:name "containerOfExpression"@en ;
    reg:status <http://metadataregistry.org/uri/RegStatus/1001> ;
    rdfs:domain <http://rdaregistry.info/Elements/c/C10006> ;
    rdfs:isDefinedBy <http://rdaregistry.info/Elements/e/> ;
    rdfs:subPropertyOf <http://rdaregistry.info/Elements/e/P20236> ;
    skos:definition "Relates an expression to an expression of a work that is a discrete component of a larger expression."@en .

<http://rdaregistry.info/Elements/e/P20146> a rdf:Property ;
    rdfs:label "is errata to (expression)"@en ;
    rdakit:instructionNumber "24.5" ;
    rdakit:toolkitDefinition "An expression of a work that is augmented by a list of errors in a predominant work, discovered after publication, with their corrections."@en,
        "Una expresión de una obra que es aumentada por una lista de errores en la obra principal, descubiertos después de la publicación, con sus correcciones."@es,
        "Expression d’une œuvre qui est augmentée d’une liste d’erreurs dans l’œuvre prédominante, découvertes après publication, avec leurs corrections."@fr ;
    rdakit:toolkitLabel "errata to (expression)"@en,
        "fe de erratas de (expresión)"@es,
        "errata de (expression)"@fr ;
    reg:hasSubproperty <http://rdaregistry.info/Elements/e/object/P20146> ;
    reg:hasUnconstrained <http://rdaregistry.info/Elements/u/P60251> ;
    reg:lexicalAlias <http://rdaregistry.info/Elements/e/errataToExpression.en> ;
    reg:name "errataToExpression"@en ;
    reg:status <http://metadataregistry.org/uri/RegStatus/1001> ;
    rdfs:domain <http://rdaregistry.info/Elements/c/C10006> ;
    rdfs:isDefinedBy <http://rdaregistry.info/Elements/e/> ;
    rdfs:subPropertyOf <http://rdaregistry.info/Elements/e/P20192> ;
    skos:definition "Relates an expression to an expression of a work that is augmented by a list of errors in a predominant work, discovered after publication, with their corrections."@en .

<http://rdaregistry.info/Elements/e/P20147> a rdf:Property ;
    rdfs:label "is guide to (expression)"@en ;
    rdakit:instructionNumber "24.5" ;
    rdakit:toolkitDefinition "An expression of a work that is augmented by another work consisting of material to help the user of a predominant work, such as notes, learning and study aids, exercises, problems, questions and answers, instructor or student materials, etc."@en,
        "Una expresión de una obra que es aumentada por otra obra que consiste en material de ayuda para el usuario de la obra principal, tal como notas, ayudas de aprendizaje y estudio, ejercicios, problemas, preguntas y respuestas, materiales para el instructor y el estudiante, etc."@es,
        "Expression d’une œuvre qui est augmentée par une autre œuvre consistant en documentation destinée à aider l’utilisateur de l’œuvre prédominante, telle que des notes, des outils pédagogiques, des exercices, des problèmes, des questions et réponses, du matériel didactique, etc."@fr ;
    rdakit:toolkitLabel "guide to (expression)"@en,
        "guía de (expresión)"@es,
        "guide de (expression)"@fr ;
    reg:hasSubproperty <http://rdaregistry.info/Elements/e/object/P20147> ;
    reg:hasUnconstrained <http://rdaregistry.info/Elements/u/P60252> ;
    reg:lexicalAlias <http://rdaregistry.info/Elements/e/guideToExpression.en> ;
    reg:name "guideToExpression"@en ;
    reg:status <http://metadataregistry.org/uri/RegStatus/1001> ;
    rdfs:domain <http://rdaregistry.info/Elements/c/C10006> ;
    rdfs:isDefinedBy <http://rdaregistry.info/Elements/e/> ;
    rdfs:subPropertyOf <http://rdaregistry.info/Elements/e/P20192> ;
    skos:definition "Relates an expression to an expression of a work that is augmented by another work consisting of material to help the user of a predominant work, such as notes, learning and study aids, exercises, problems, questions and answers, instructor or student materials, etc."@en .

<http://rdaregistry.info/Elements/e/P20148> a rdf:Property ;
    rdfs:label "is illustrations for (expression)"@en ;
    rdakit:instructionNumber "24.5" ;
    rdakit:toolkitDefinition "An expression of a work that is augmented by pictorial content designed to explain or decorate it."@en,
        "Una expresión de una obra que es aumentada con contenido pictórico diseñado para explicarla o decorarla."@es,
        "Expression d’une œuvre qui est augmentée par du contenu visuel destiné à l’expliquer ou à la décorer."@fr ;
    rdakit:toolkitLabel "illustrations for (expression)"@en,
        "ilustraciones para (expresión)"@es,
        "illustrations pour (expression)"@fr ;
    reg:hasSubproperty <http://rdaregistry.info/Elements/e/object/P20148> ;
    reg:hasUnconstrained <http://rdaregistry.info/Elements/u/P60254> ;
    reg:lexicalAlias <http://rdaregistry.info/Elements/e/illustrationsForExpression.en> ;
    reg:name "illustrationsForExpression"@en ;
    reg:status <http://metadataregistry.org/uri/RegStatus/1001> ;
    rdfs:domain <http://rdaregistry.info/Elements/c/C10006> ;
    rdfs:isDefinedBy <http://rdaregistry.info/Elements/e/> ;
    rdfs:subPropertyOf <http://rdaregistry.info/Elements/e/P20192> ;
    skos:definition "Relates an expression to an expression of a work that is augmented by pictorial content designed to explain or decorate it."@en .

<http://rdaregistry.info/Elements/e/P20149> a rdf:Property ;
    rdfs:label "is continuation of (expression)"@en ;
    rdakit:instructionNumber "24.5" ;
    rdakit:toolkitDefinition "An expression of a work that is continued by the content of an expression of a later work."@en,
        "Una expresión de una obra que es continuada por el contenido de una expresión de una obra posterior."@es,
        "Expression d’une œuvre qui est continuée par le contenu d’une expression d’une œuvre ultérieure."@fr ;
    rdakit:toolkitLabel "continuation of (expression)"@en,
        "continuación de (expresión)"@es,
        "continuation de (expression)"@fr ;
    reg:hasSubproperty <http://rdaregistry.info/Elements/e/object/P20149> ;
    reg:hasUnconstrained <http://rdaregistry.info/Elements/u/P60576> ;
    reg:lexicalAlias <http://rdaregistry.info/Elements/e/continuationOfExpression.en> ;
    reg:name "continuationOfExpression"@en ;
    reg:status <http://metadataregistry.org/uri/RegStatus/1001> ;
    rdfs:domain <http://rdaregistry.info/Elements/c/C10006> ;
    rdfs:isDefinedBy <http://rdaregistry.info/Elements/e/> ;
    rdfs:subPropertyOf <http://rdaregistry.info/Elements/e/P20154> ;
    skos:definition "Relates an expression to an expression of a work that is continued by the content of an expression of a later work."@en ;
    skos:scopeNote "This relationship applies generally to serials."@en .

<http://rdaregistry.info/Elements/e/P20150> a rdf:Property ;
    reg:status <http://metadataregistry.org/uri/RegStatus/1008> ;
    rdfs:isDefinedBy <http://rdaregistry.info/Elements/e/> ;
    rdfs:subPropertyOf <http://rdaregistry.info/Elements/e/P20072> .

<http://rdaregistry.info/Elements/e/P20151> a rdf:Property ;
    rdfs:label "is supplement to (expression)"@en ;
    rdakit:instructionNumber "24.5" ;
    rdakit:toolkitDefinition "An expression of a work that is updated or otherwise complemented by an augmenting expression."@en,
        "Una expresión de una obra que es actualizada o complementada por la expresión que aumenta."@es,
        "Expression d’une œuvre qui est mise à jour ou complétée d’une autre façon par l’expression augmentante."@fr ;
    rdakit:toolkitLabel "supplement to (expression)"@en,
        "suplemento de (expresión)"@es,
        "supplément de (expression)"@fr ;
    reg:hasSubproperty <http://rdaregistry.info/Elements/e/object/P20151> ;
    reg:hasUnconstrained <http://rdaregistry.info/Elements/u/P60259> ;
    reg:lexicalAlias <http://rdaregistry.info/Elements/e/supplementToExpression.en> ;
    reg:name "supplementToExpression"@en ;
    reg:status <http://metadataregistry.org/uri/RegStatus/1001> ;
    rdfs:domain <http://rdaregistry.info/Elements/c/C10006> ;
    rdfs:isDefinedBy <http://rdaregistry.info/Elements/e/> ;
    rdfs:subPropertyOf <http://rdaregistry.info/Elements/e/P20192> ;
    skos:definition "Relates an expression to an expression of a work that is updated or otherwise complemented by an augmenting expression."@en .

<http://rdaregistry.info/Elements/e/P20155> a rdf:Property ;
    rdfs:label "is finding aid (expression)"@en ;
    rdakit:instructionNumber "24.5" ;
    rdakit:toolkitDefinition "An expression of a work that provides a guide to the organization, arrangement, and contents of an archival collection."@en,
        "Una expresión de una obra que proporciona una guía para la organización, ordenación y contenido de una colección archivística."@es,
        "Expression d’une œuvre qui fournit un guide de l’organisation, du classement et du contenu d’une collection ou d’un fonds d’archives."@fr ;
    rdakit:toolkitLabel "finding aid (expression)"@en,
        "guía de búsqueda (expresión)"@es,
        "instrument de recherche (expression)"@fr ;
    reg:hasSubproperty <http://rdaregistry.info/Elements/e/object/P20155> ;
    reg:hasUnconstrained <http://rdaregistry.info/Elements/u/P60262> ;
    reg:lexicalAlias <http://rdaregistry.info/Elements/e/findingAidExpression.en> ;
    reg:name "findingAidExpression"@en ;
    reg:status <http://metadataregistry.org/uri/RegStatus/1001> ;
    rdfs:domain <http://rdaregistry.info/Elements/c/C10006> ;
    rdfs:isDefinedBy <http://rdaregistry.info/Elements/e/> ;
    rdfs:subPropertyOf <http://rdaregistry.info/Elements/e/P20105> ;
    skos:definition "Relates an expression to an expression of a work that provides a guide to the organization, arrangement, and contents of an archival collection."@en .

<http://rdaregistry.info/Elements/e/P20156> a rdf:Property ;
    rdfs:label "is index (expression)"@en ;
    rdakit:instructionNumber "24.5" ;
    rdakit:toolkitDefinition "An expression of a work that provides a systematic, alphabetical guide to the contents of a predominant expression, usually keyed to page numbers or other reference codes."@en,
        "Una expresión de una obra que proporciona una guía alfabética y sistemática al contenido de la entidad principal, generalmente indicando los números de página u otros códigos de referencia."@es,
        "Expression d’une œuvre qui fournit un guide méthodique et alphabétique du contenu de l’expression prédominante, renvoyant généralement à des numéros de page ou à d’autres codes de référence."@fr ;
    rdakit:toolkitLabel "index (expression)"@en,
        "índice (expresión)"@es,
        "index (expression)"@fr ;
    reg:hasSubproperty <http://rdaregistry.info/Elements/e/object/P20156> ;
    reg:hasUnconstrained <http://rdaregistry.info/Elements/u/P60263> ;
    reg:lexicalAlias <http://rdaregistry.info/Elements/e/indexExpression.en> ;
    reg:name "indexExpression"@en ;
    reg:status <http://metadataregistry.org/uri/RegStatus/1001> ;
    rdfs:domain <http://rdaregistry.info/Elements/c/C10006> ;
    rdfs:isDefinedBy <http://rdaregistry.info/Elements/e/> ;
    rdfs:subPropertyOf <http://rdaregistry.info/Elements/e/P20105> ;
    skos:definition "Relates an expression to an expression of a work that provides a systematic, alphabetical guide to the contents of a predominant expression, usually keyed to page numbers or other reference codes."@en .

<http://rdaregistry.info/Elements/e/P20158> a rdf:Property ;
    rdfs:label "is motion picture screenplay (expression)"@en ;
    rdakit:instructionNumber "24.5" ;
    rdakit:toolkitDefinition "An expression of a work that provides text for a motion picture."@en,
        "Una expresión de una obra que proporciona el texto para una película cinematográfica."@es,
        "Expression d’une œuvre qui fournit le texte d’un film."@fr ;
    rdakit:toolkitLabel "motion picture screenplay (expression)"@en,
        "guión cinematográfico (expresión)"@es,
        "scénario de film (expression)"@fr ;
    reg:hasSubproperty <http://rdaregistry.info/Elements/e/object/P20158> ;
    reg:hasUnconstrained <http://rdaregistry.info/Elements/u/P60265> ;
    reg:lexicalAlias <http://rdaregistry.info/Elements/e/motionPictureScreenplayExpression.en> ;
    reg:name "motionPictureScreenplayExpression"@en ;
    reg:status <http://metadataregistry.org/uri/RegStatus/1001> ;
    rdfs:domain <http://rdaregistry.info/Elements/c/C10006> ;
    rdfs:isDefinedBy <http://rdaregistry.info/Elements/e/> ;
    rdfs:subPropertyOf <http://rdaregistry.info/Elements/e/P20157> ;
    skos:definition "Relates an expression to an expression of a work that provides text for a motion picture."@en .

<http://rdaregistry.info/Elements/e/P20159> a rdf:Property ;
    rdfs:label "is musical setting of (expression)"@en ;
    rdakit:instructionNumber "24.5" ;
    rdakit:toolkitDefinition "An expression of a work that provides text for a non-dramatic musical work, other than an oratorio."@en,
        "Una expresión de una obra que proporciona el texto de una obra musical no dramática, diferente de un oratorio."@es,
        "Expression d’une œuvre qui fournit le texte d’une œuvre musicale non théâtrale, autre qu’un oratorio."@fr ;
    rdakit:toolkitLabel "musical setting of (expression)"@en,
        "composición musical de (expresión)"@es,
        "mise en musique de (expression)"@fr ;
    reg:hasSubproperty <http://rdaregistry.info/Elements/e/object/P20159> ;
    reg:hasUnconstrained <http://rdaregistry.info/Elements/u/P60266> ;
    reg:lexicalAlias <http://rdaregistry.info/Elements/e/musicalSettingOfExpression.en> ;
    reg:name "musicalSettingOfExpression"@en ;
    reg:status <http://metadataregistry.org/uri/RegStatus/1001> ;
    rdfs:domain <http://rdaregistry.info/Elements/c/C10006> ;
    rdfs:isDefinedBy <http://rdaregistry.info/Elements/e/> ;
    rdfs:subPropertyOf <http://rdaregistry.info/Elements/e/P20204> ;
    skos:definition "Relates an expression to an expression of a work that provides text for a non-dramatic musical work, other than an oratorio."@en .

<http://rdaregistry.info/Elements/e/P20160> a rdf:Property ;
    rdfs:label "is radio script (expression)"@en ;
    rdakit:instructionNumber "24.5" ;
    rdakit:toolkitDefinition "An expression of a work that provides text for a radio program."@en,
        "Una expresión de una obra que proporciona el texto para un programa de radio."@es,
        "Expression d’une œuvre qui fournit le texte d’une émission de radio."@fr ;
    rdakit:toolkitLabel "radio script (expression)"@en,
        "guión radiofónico (expresión)"@es,
        "script radiophonique (expression)"@fr ;
    reg:hasSubproperty <http://rdaregistry.info/Elements/e/object/P20160> ;
    reg:hasUnconstrained <http://rdaregistry.info/Elements/u/P60267> ;
    reg:lexicalAlias <http://rdaregistry.info/Elements/e/radioScriptExpression.en> ;
    reg:name "radioScriptExpression"@en ;
    reg:status <http://metadataregistry.org/uri/RegStatus/1001> ;
    rdfs:domain <http://rdaregistry.info/Elements/c/C10006> ;
    rdfs:isDefinedBy <http://rdaregistry.info/Elements/e/> ;
    rdfs:subPropertyOf <http://rdaregistry.info/Elements/e/P20100> ;
    skos:definition "Relates an expression to an expression of a work that provides text for a radio program."@en .

<http://rdaregistry.info/Elements/e/P20161> a rdf:Property ;
    rdfs:label "is television screenplay (expression)"@en ;
    rdakit:instructionNumber "24.5" ;
    rdakit:toolkitDefinition "An expression of a work that provides text for a television program."@en,
        "Una expresión de una obra que proporciona el texto para un programa de televisión."@es,
        "Expression d’une œuvre qui fournit le texte d’une émission de télévision."@fr ;
    rdakit:toolkitLabel "television screenplay (expression)"@en,
        "guión para televisión (expresión) Una"@es,
        "scénario de télévision (expression)"@fr ;
    reg:hasSubproperty <http://rdaregistry.info/Elements/e/object/P20161> ;
    reg:hasUnconstrained <http://rdaregistry.info/Elements/u/P60268> ;
    reg:lexicalAlias <http://rdaregistry.info/Elements/e/televisionScreenplayExpression.en> ;
    reg:name "televisionScreenplayExpression"@en ;
    reg:status <http://metadataregistry.org/uri/RegStatus/1001> ;
    rdfs:domain <http://rdaregistry.info/Elements/c/C10006> ;
    rdfs:isDefinedBy <http://rdaregistry.info/Elements/e/> ;
    rdfs:subPropertyOf <http://rdaregistry.info/Elements/e/P20157> ;
    skos:definition "Relates an expression to an expression of a work that provides text for a television program."@en .

<http://rdaregistry.info/Elements/e/P20162> a rdf:Property ;
    rdfs:label "is video screenplay (expression)"@en ;
    rdakit:instructionNumber "24.5" ;
    rdakit:toolkitDefinition "An expression of a work that provides text for a video."@en,
        "Una expresión de una obra que proporciona el texto para un video."@es,
        "Expression d’une œuvre qui fournit le texte d’une vidéo."@fr ;
    rdakit:toolkitLabel "video screenplay (expression)"@en,
        "guión para video (expresión)"@es,
        "scénario de vidéo (expression)"@fr ;
    reg:hasSubproperty <http://rdaregistry.info/Elements/e/object/P20162> ;
    reg:hasUnconstrained <http://rdaregistry.info/Elements/u/P60269> ;
    reg:lexicalAlias <http://rdaregistry.info/Elements/e/videoScreenplayExpression.en> ;
    reg:name "videoScreenplayExpression"@en ;
    reg:status <http://metadataregistry.org/uri/RegStatus/1001> ;
    rdfs:domain <http://rdaregistry.info/Elements/c/C10006> ;
    rdfs:isDefinedBy <http://rdaregistry.info/Elements/e/> ;
    rdfs:subPropertyOf <http://rdaregistry.info/Elements/e/P20157> ;
    skos:definition "Relates an expression to an expression of a work that provides text for a video."@en .

<http://rdaregistry.info/Elements/e/P20163> a rdf:Property ;
    rdfs:label "is libretto (expression)"@en ;
    rdakit:instructionNumber "24.5" ;
    rdakit:toolkitDefinition "An expression of a work that provides the text of an opera or other work for the musical stage, or an oratorio."@en,
        "Una expresión de una obra que proporciona el texto de una ópera u otra obra para representación musical, o un oratorio."@es,
        "Expression d’une œuvre qui fournit le texte d’un opéra ou d’une autre œuvre pour la scène musicale, ou bien d’un oratorio."@fr ;
    rdakit:toolkitLabel "libretto (expression)"@en,
        "libreto (expresión)"@es,
        "livret (expression)"@fr ;
    reg:hasSubproperty <http://rdaregistry.info/Elements/e/object/P20163> ;
    reg:hasUnconstrained <http://rdaregistry.info/Elements/u/P60270> ;
    reg:lexicalAlias <http://rdaregistry.info/Elements/e/librettoExpression.en> ;
    reg:name "librettoExpression"@en ;
    reg:status <http://metadataregistry.org/uri/RegStatus/1001> ;
    rdfs:domain <http://rdaregistry.info/Elements/c/C10006> ;
    rdfs:isDefinedBy <http://rdaregistry.info/Elements/e/> ;
    rdfs:subPropertyOf <http://rdaregistry.info/Elements/e/P20100> ;
    skos:definition "Relates an expression to an expression of a work that provides the text of an opera or other work for the musical stage, or an oratorio."@en .

<http://rdaregistry.info/Elements/e/P20164> a rdf:Property ;
    rdfs:label "is paraphrased as (expression)"@en ;
    rdakit:instructionNumber "24.5" ;
    rdakit:toolkitDefinition "An expression of a work that restates the content of a source work in a different form."@en,
        "Una expresión de una obra que replantea el contenido de una obra fuente en una forma diferente."@es,
        "Expression d’une œuvre qui reprend le contenu de l’œuvre source sous une formulation différente."@fr ;
    rdakit:toolkitLabel "paraphrased as (expression)"@en,
        "parafraseada como (expresión)"@es,
        "paraphrasé comme (expression)"@fr ;
    reg:hasSubproperty <http://rdaregistry.info/Elements/e/object/P20164> ;
    reg:hasUnconstrained <http://rdaregistry.info/Elements/u/P60273> ;
    reg:lexicalAlias <http://rdaregistry.info/Elements/e/paraphrasedAsExpression.en> ;
    reg:name "paraphrasedAsExpression"@en ;
    reg:status <http://metadataregistry.org/uri/RegStatus/1001> ;
    rdfs:domain <http://rdaregistry.info/Elements/c/C10006> ;
    rdfs:isDefinedBy <http://rdaregistry.info/Elements/e/> ;
    rdfs:subPropertyOf <http://rdaregistry.info/Elements/e/P20203> ;
    skos:definition "Relates an expression to an expression of a work that restates the content of a source work in a different form."@en .

<http://rdaregistry.info/Elements/e/P20165> a rdf:Property ;
    rdfs:label "is arranged as"@en ;
    rdakit:instructionNumber "24.5" ;
    rdakit:toolkitDefinition "An expression of a musical work that rewrites a source expression for a medium of performance different from that for which the work was originally intended."@en,
        "Una expresión de una obra que reescribe la expresión fuente para un medio de interpretación diferente de aquel para el cual fue prevista originalmente."@es,
        "Expression d’une œuvre musicale qui réécrit l’expression source pour une distribution d’exécution différente de celle à laquelle l’œuvre était destinée à l’origine."@fr ;
    rdakit:toolkitLabel "arranged as"@en,
        "arreglada como"@es,
        "arrangé comme"@fr ;
    reg:hasSubproperty <http://rdaregistry.info/Elements/e/object/P20165> ;
    reg:hasUnconstrained <http://rdaregistry.info/Elements/u/P60274> ;
    reg:lexicalAlias <http://rdaregistry.info/Elements/e/arrangedAs.en> ;
    reg:name "arrangedAs"@en ;
    reg:status <http://metadataregistry.org/uri/RegStatus/1001> ;
    rdfs:domain <http://rdaregistry.info/Elements/c/C10006> ;
    rdfs:isDefinedBy <http://rdaregistry.info/Elements/e/> ;
    rdfs:subPropertyOf <http://rdaregistry.info/Elements/e/P20203> ;
    skos:definition "Relates an expression to an expression of a musical work that rewrites a source expression for a medium of performance different from that for which the work was originally intended."@en .

<http://rdaregistry.info/Elements/e/P20166> a rdf:Property ;
    rdfs:label "is abridged as (expression)"@en ;
    rdakit:instructionNumber "24.5" ;
    rdakit:toolkitDefinition "An expression of a work that shortens a source expression without changing the general meaning or manner of presentation."@en,
        "Una expresión de una obra que acorta la entidad fuente sin cambiar el sentido general o la forma de presentación."@es,
        "Expression d’une œuvre qui raccourcit l’expression source sans en changer le sens général ou le mode de présentation."@fr ;
    rdakit:toolkitLabel "abridged as (expression)"@en,
        "abreviada como (expresión)"@es,
        "abrégé comme (expression)"@fr ;
    reg:hasSubproperty <http://rdaregistry.info/Elements/e/object/P20166> ;
    reg:hasUnconstrained <http://rdaregistry.info/Elements/u/P60275> ;
    reg:lexicalAlias <http://rdaregistry.info/Elements/e/abridgedAsExpression.en> ;
    reg:name "abridgedAsExpression"@en ;
    reg:status <http://metadataregistry.org/uri/RegStatus/1001> ;
    rdfs:domain <http://rdaregistry.info/Elements/c/C10006> ;
    rdfs:isDefinedBy <http://rdaregistry.info/Elements/e/> ;
    rdfs:subPropertyOf <http://rdaregistry.info/Elements/e/P20203> ;
    skos:definition "Relates an expression to an expression of a work that shortens a source expression without changing the general meaning or manner of presentation."@en .

<http://rdaregistry.info/Elements/e/P20167> a rdf:Property ;
    rdfs:label "is continuation in part of (expression)"@en ;
    rdakit:instructionNumber "24.5" ;
    rdakit:toolkitDefinition "An expression of a work that split into two or more separate expressions with new titles."@en,
        "Una expresión de una obra que se divide en dos o más entidades separadas con nuevos títulos."@es,
        "Expression d’une œuvre qui s’est scindée en deux ou plusieurs expressions distinctes avec de nouveaux titres."@fr ;
    rdakit:toolkitLabel "continuation in part of (expression)"@en,
        "continúa en parte (expresión)"@es,
        "continuation partielle de (expression)"@fr ;
    reg:hasSubproperty <http://rdaregistry.info/Elements/e/object/P20167> ;
    reg:hasUnconstrained <http://rdaregistry.info/Elements/u/P60276> ;
    reg:lexicalAlias <http://rdaregistry.info/Elements/e/continuationInPartOfExpression.en> ;
    reg:name "continuationInPartOfExpression"@en ;
    reg:status <http://metadataregistry.org/uri/RegStatus/1001> ;
    rdfs:domain <http://rdaregistry.info/Elements/c/C10006> ;
    rdfs:isDefinedBy <http://rdaregistry.info/Elements/e/> ;
    rdfs:subPropertyOf <http://rdaregistry.info/Elements/e/P20154> ;
    skos:definition "Relates an expression to an expression of a work that split into two or more separate expressions with new titles."@en ;
    skos:scopeNote "This relationship applies generally to serials."@en .

<http://rdaregistry.info/Elements/e/P20168> a rdf:Property ;
    rdfs:label "is separated from (expression)"@en ;
    rdakit:instructionNumber "24.5" ;
    rdakit:toolkitDefinition "An expression of a work that spun off a part of its content to form a new expression."@en,
        "Una expresión de una obra que se desprende de una parte de su contenido para formar una expresión nueva."@es,
        "Expression d’une œuvre dont une partie du contenu a été détachée pour former une nouvelle expression."@fr ;
    rdakit:toolkitLabel "separated from (expression)"@en,
        "separada de (expresión)"@es,
        "scission de (expression)"@fr ;
    reg:hasSubproperty <http://rdaregistry.info/Elements/e/object/P20168> ;
    reg:hasUnconstrained <http://rdaregistry.info/Elements/u/P60277> ;
    reg:lexicalAlias <http://rdaregistry.info/Elements/e/separatedFromExpression.en> ;
    reg:name "separatedFromExpression"@en ;
    reg:status <http://metadataregistry.org/uri/RegStatus/1001> ;
    rdfs:domain <http://rdaregistry.info/Elements/c/C10006> ;
    rdfs:isDefinedBy <http://rdaregistry.info/Elements/e/> ;
    rdfs:subPropertyOf <http://rdaregistry.info/Elements/e/P20154> ;
    skos:definition "Relates an expression to an expression of a work that spun off a part of its content to form a new expression."@en .

<http://rdaregistry.info/Elements/e/P20170> a rdf:Property ;
    rdfs:label "is digested as (expression)"@en ;
    rdakit:instructionNumber "24.5" ;
    rdakit:toolkitDefinition "An expression of a work that systematically and comprehensively condenses a source expression."@en,
        "Una expresión de una obra que sistemática e integralmente condensa la expresión fuente."@es,
        "Expression d’une œuvre qui abrège de manière systématique et complète l’expression source."@fr ;
    rdakit:toolkitLabel "digested as (expression)"@en,
        "compendiada como (expresión)"@es,
        "condensé comme (expression)"@fr ;
    reg:hasSubproperty <http://rdaregistry.info/Elements/e/object/P20170> ;
    reg:hasUnconstrained <http://rdaregistry.info/Elements/u/P60279> ;
    reg:lexicalAlias <http://rdaregistry.info/Elements/e/digestedAsExpression.en> ;
    reg:name "digestedAsExpression"@en ;
    reg:status <http://metadataregistry.org/uri/RegStatus/1001> ;
    rdfs:domain <http://rdaregistry.info/Elements/c/C10006> ;
    rdfs:isDefinedBy <http://rdaregistry.info/Elements/e/> ;
    rdfs:subPropertyOf <http://rdaregistry.info/Elements/e/P20203> ;
    skos:definition "Relates an expression to an expression of a work that systematically and comprehensively condenses a source expression."@en .

<http://rdaregistry.info/Elements/e/P20172> a rdf:Property ;
    rdfs:label "is supplement (expression)"@en ;
    rdakit:instructionNumber "24.5" ;
    rdakit:toolkitDefinition "An expression of a work that updates or otherwise complements a predominant expression."@en,
        "Una expresión de una obra que actualiza o complementa la expresión principal."@es,
        "Expression d’une œuvre qui met à jour ou complète d’une autre façon l’expression prédominante."@fr ;
    rdakit:toolkitLabel "supplement (expression)"@en,
        "suplemento (expresión)"@es,
        "supplément (expression)"@fr ;
    reg:hasSubproperty <http://rdaregistry.info/Elements/e/object/P20172> ;
    reg:hasUnconstrained <http://rdaregistry.info/Elements/u/P60281> ;
    reg:lexicalAlias <http://rdaregistry.info/Elements/e/supplementExpression.en> ;
    reg:name "supplementExpression"@en ;
    reg:status <http://metadataregistry.org/uri/RegStatus/1001> ;
    rdfs:domain <http://rdaregistry.info/Elements/c/C10006> ;
    rdfs:isDefinedBy <http://rdaregistry.info/Elements/e/> ;
    rdfs:subPropertyOf <http://rdaregistry.info/Elements/e/P20105> ;
    skos:definition "Relates an expression to an expression of a work that updates or otherwise complements a predominant expression."@en .

<http://rdaregistry.info/Elements/e/P20173> a rdf:Property ;
    rdfs:label "is screenplay for motion picture (expression)"@en ;
    rdakit:instructionNumber "24.5" ;
    rdakit:toolkitDefinition "An expression of a work that uses the text as a screenplay for a motion picture."@en,
        "Una expresión de una obra que utiliza el texto como un guión para una película cinematográfica."@es,
        "Expression d’une œuvre qui utilise le texte comme scénario d’un film."@fr ;
    rdakit:toolkitLabel "screenplay for motion picture (expression)"@en,
        "guión para la película cinematográfica (expresión)"@es,
        "scénario pour le film (expression)"@fr ;
    reg:hasSubproperty <http://rdaregistry.info/Elements/e/object/P20173> ;
    reg:hasUnconstrained <http://rdaregistry.info/Elements/u/P60282> ;
    reg:lexicalAlias <http://rdaregistry.info/Elements/e/screenplayForMotionPictureExpression.en> ;
    reg:name "screenplayForMotionPictureExpression"@en ;
    reg:status <http://metadataregistry.org/uri/RegStatus/1001> ;
    rdfs:domain <http://rdaregistry.info/Elements/c/C10006> ;
    rdfs:isDefinedBy <http://rdaregistry.info/Elements/e/> ;
    rdfs:subPropertyOf <http://rdaregistry.info/Elements/e/P20102> ;
    skos:definition "Relates an expression to an expression of a work that uses the text as a screenplay for a motion picture."@en .

<http://rdaregistry.info/Elements/e/P20174> a rdf:Property ;
    rdfs:label "is screenplay for television program (expression)"@en ;
    rdakit:instructionNumber "24.5" ;
    rdakit:toolkitDefinition "An expression of a work that uses the text as a screenplay for a television program."@en,
        "Una expresión de una obra que utiliza el texto como un guión para un programa de televisión."@es,
        "Expression d’une œuvre qui utilise le texte comme scénario d’une émission de télévision."@fr ;
    rdakit:toolkitLabel "screenplay for television program (expression)"@en,
        "guión para el programa de televisión (expresión)"@es,
        "scénario pour l’émission de télévision (expression)"@fr ;
    reg:hasSubproperty <http://rdaregistry.info/Elements/e/object/P20174> ;
    reg:hasUnconstrained <http://rdaregistry.info/Elements/u/P60283> ;
    reg:lexicalAlias <http://rdaregistry.info/Elements/e/screenplayForTelevisionProgramExpression.en> ;
    reg:name "screenplayForTelevisionProgramExpression"@en ;
    reg:status <http://metadataregistry.org/uri/RegStatus/1001> ;
    rdfs:domain <http://rdaregistry.info/Elements/c/C10006> ;
    rdfs:isDefinedBy <http://rdaregistry.info/Elements/e/> ;
    rdfs:subPropertyOf <http://rdaregistry.info/Elements/e/P20102> ;
    skos:definition "Relates an expression to an expression of a work that uses the text as a screenplay for a television program."@en .

<http://rdaregistry.info/Elements/e/P20175> a rdf:Property ;
    rdfs:label "is screenplay for video (expression)"@en ;
    rdakit:instructionNumber "24.5" ;
    rdakit:toolkitDefinition "An expression of a work that uses the text as a screenplay for a video."@en,
        "Una expresión de una obra que utiliza el texto como un guión para un video."@es,
        "Expression d’une œuvre qui utilise le texte comme scénario d’une vidéo."@fr ;
    rdakit:toolkitLabel "screenplay for video (expression)"@en,
        "guión para el video (expresión)"@es,
        "scénario pour la vidéo (expression)"@fr ;
    reg:hasSubproperty <http://rdaregistry.info/Elements/e/object/P20175> ;
    reg:hasUnconstrained <http://rdaregistry.info/Elements/u/P60284> ;
    reg:lexicalAlias <http://rdaregistry.info/Elements/e/screenplayForVideoExpression.en> ;
    reg:name "screenplayForVideoExpression"@en ;
    reg:status <http://metadataregistry.org/uri/RegStatus/1001> ;
    rdfs:domain <http://rdaregistry.info/Elements/c/C10006> ;
    rdfs:isDefinedBy <http://rdaregistry.info/Elements/e/> ;
    rdfs:subPropertyOf <http://rdaregistry.info/Elements/e/P20102> ;
    skos:definition "Relates an expression to an expression of a work that uses the text as a screenplay for a video."@en .

<http://rdaregistry.info/Elements/e/P20176> a rdf:Property ;
    rdfs:label "is script for radio program (expression)"@en ;
    rdakit:instructionNumber "24.5" ;
    rdakit:toolkitDefinition "An expression of a work that uses the text as a script for a radio program."@en,
        "Una expresión de una obra que utiliza el texto de la obra fuente como el guión para un programa radiofónico."@es,
        "Expression d’une œuvre qui utilise le texte de l’œuvre source comme script d’une émission de radio."@fr ;
    rdakit:toolkitLabel "script for radio program (expression)"@en,
        "guión para el programa de radio (expresión)"@es,
        "script pour l’émission de radio (expression)"@fr ;
    reg:hasSubproperty <http://rdaregistry.info/Elements/e/object/P20176> ;
    reg:hasUnconstrained <http://rdaregistry.info/Elements/u/P60285> ;
    reg:lexicalAlias <http://rdaregistry.info/Elements/e/scriptForRadioProgramExpression.en> ;
    reg:name "scriptForRadioProgramExpression"@en ;
    reg:status <http://metadataregistry.org/uri/RegStatus/1001> ;
    rdfs:domain <http://rdaregistry.info/Elements/c/C10006> ;
    rdfs:isDefinedBy <http://rdaregistry.info/Elements/e/> ;
    rdfs:subPropertyOf <http://rdaregistry.info/Elements/e/P20100> ;
    skos:definition "Relates an expression to an expression of a work that uses the text as a script for a radio program."@en .

<http://rdaregistry.info/Elements/e/P20177> a rdf:Property ;
    rdfs:label "is addenda to (expression)"@en ;
    rdakit:instructionNumber "24.5" ;
    rdakit:toolkitDefinition "An expression of a work whose content is completed with brief content from an expression of another work."@en,
        "Una expresión de una obra a la cual es añadido material adicional, menos extenso que un suplemento, pero esencial para la integridad del contenido de la obra; es añadido generalmente al final del contenido pero algunas veces se publica separadamente."@es,
        "Expression d’une œuvre à laquelle sont ajoutées de brèves informations additionnelles, moins étendues qu’un supplément, mais essentielles à la complétude du contenu de l’œuvre ; ces informations sont généralement ajoutées à la fin du contenu, mais peuvent aussi parfois être publiées séparément."@fr ;
    rdakit:toolkitLabel "addenda to (expression)"@en,
        "adenda de (expresión)"@es,
        "addenda de (expression)"@fr ;
    reg:hasSubproperty <http://rdaregistry.info/Elements/e/object/P20177> ;
    reg:hasUnconstrained <http://rdaregistry.info/Elements/u/P60286> ;
    reg:lexicalAlias <http://rdaregistry.info/Elements/e/addendaToExpression.en> ;
    reg:name "addendaToExpression"@en ;
    reg:status <http://metadataregistry.org/uri/RegStatus/1001> ;
    rdfs:domain <http://rdaregistry.info/Elements/c/C10006> ;
    rdfs:isDefinedBy <http://rdaregistry.info/Elements/e/> ;
    rdfs:subPropertyOf <http://rdaregistry.info/Elements/e/P20192> ;
    skos:definition "Relates an expression to an expression of a work whose content is completed with brief content from an expression of another work."@en .

<http://rdaregistry.info/Elements/e/P20178> a rdf:Property ;
    reg:status <http://metadataregistry.org/uri/RegStatus/1008> ;
    rdfs:isDefinedBy <http://rdaregistry.info/Elements/e/> ;
    rdfs:subPropertyOf <http://rdaregistry.info/Elements/e/P20072> .

<http://rdaregistry.info/Elements/e/P20179> a rdf:Property ;
    rdfs:label "is summary of (expression)"@en ;
    rdakit:instructionNumber "24.5" ;
    rdakit:toolkitDefinition "An expression of a work used as the basis for a brief recapitulation of its content."@en,
        "Una expresión de una obra usada como base para una recapitulación breve de su contenido."@es,
        "Expression d’une œuvre servant de base à une brève récapitulation de son contenu."@fr ;
    rdakit:toolkitLabel "summary of (expression)"@en,
        "sumario de (expresión)"@es,
        "résumé de (expression)"@fr ;
    reg:hasSubproperty <http://rdaregistry.info/Elements/e/object/P20179> ;
    reg:hasUnconstrained <http://rdaregistry.info/Elements/u/P60289> ;
    reg:lexicalAlias <http://rdaregistry.info/Elements/e/summaryOfExpression.en> ;
    reg:name "summaryOfExpression"@en ;
    reg:status <http://metadataregistry.org/uri/RegStatus/1001> ;
    rdfs:domain <http://rdaregistry.info/Elements/c/C10006> ;
    rdfs:isDefinedBy <http://rdaregistry.info/Elements/e/> ;
    rdfs:subPropertyOf <http://rdaregistry.info/Elements/e/P20204> ;
    skos:definition "Relates an expression to an expression of a work used as the basis for a brief recapitulation of its content."@en .

<http://rdaregistry.info/Elements/e/P20180> a rdf:Property ;
    rdfs:label "is catalogue of (expression)"@en ;
    rdakit:instructionNumber "24.5" ;
    rdakit:toolkitDefinition "An expression of a work used as the basis for a catalogue, i.e., a complete enumeration of items arranged systematically."@en,
        "Una expresión de una obra utilizada como base para un catálogo, i.e., una enumeración completa de ítems ordenados sistemáticamente."@es,
        "Expression d’une œuvre servant de base à un catalogue, c’est-à-dire une énumération complète des items classés systématiquement."@fr ;
    rdakit:toolkitLabel "catalogue of (expression)"@en,
        "catálogo de (expresión)"@es,
        "catalogue de (expression)"@fr ;
    reg:hasSubproperty <http://rdaregistry.info/Elements/e/object/P20180> ;
    reg:hasUnconstrained <http://rdaregistry.info/Elements/u/P60290> ;
    reg:lexicalAlias <http://rdaregistry.info/Elements/e/catalogueOfExpression.en> ;
    reg:name "catalogueOfExpression"@en ;
    reg:status <http://metadataregistry.org/uri/RegStatus/1001> ;
    rdfs:domain <http://rdaregistry.info/Elements/c/C10006> ;
    rdfs:isDefinedBy <http://rdaregistry.info/Elements/e/> ;
    rdfs:subPropertyOf <http://rdaregistry.info/Elements/e/P20192> ;
    skos:definition "Relates an expression to an expression of a work used as the basis for a catalogue, i.e., a complete enumeration of items arranged systematically."@en .

<http://rdaregistry.info/Elements/e/P20181> a rdf:Property ;
    rdfs:label "is concordance to (expression)"@en ;
    rdakit:instructionNumber "24.5" ;
    rdakit:toolkitDefinition "An expression of a work used as the basis for a concordance, i.e., an index of all the words in a predominant expression."@en,
        "Una expresión de una obra utilizada como base para una concordancia, i.e., un índice de todas las palabras en la expresión principal."@es,
        "Expression d’une œuvre servant de base à une concordance, c’est-à-dire un index de tous les mots de l’expression prédominante."@fr ;
    rdakit:toolkitLabel "concordance to (expression)"@en,
        "concordancia de (expresión)"@es,
        "concordance de (expression)"@fr ;
    reg:hasSubproperty <http://rdaregistry.info/Elements/e/object/P20181> ;
    reg:hasUnconstrained <http://rdaregistry.info/Elements/u/P60291> ;
    reg:lexicalAlias <http://rdaregistry.info/Elements/e/concordanceToExpression.en> ;
    reg:name "concordanceToExpression"@en ;
    reg:status <http://metadataregistry.org/uri/RegStatus/1001> ;
    rdfs:domain <http://rdaregistry.info/Elements/c/C10006> ;
    rdfs:isDefinedBy <http://rdaregistry.info/Elements/e/> ;
    rdfs:subPropertyOf <http://rdaregistry.info/Elements/e/P20192> ;
    skos:definition "Relates an expression to an expression of a work used as the basis for a concordance, i.e., an index of all the words in a predominant expression."@en .

<http://rdaregistry.info/Elements/e/P20182> a rdf:Property ;
    reg:status <http://metadataregistry.org/uri/RegStatus/1008> ;
    rdfs:isDefinedBy <http://rdaregistry.info/Elements/e/> ;
    rdfs:subPropertyOf <http://rdaregistry.info/Elements/e/P20072> .

<http://rdaregistry.info/Elements/e/P20183> a rdf:Property ;
    rdfs:label "is choreographic adaptation of (expression)"@en ;
    rdakit:instructionNumber "24.5" ;
    rdakit:toolkitDefinition "An expression of a work that has been adapted as a work consisting of movement."@en,
        "Una expresión de una obra que ha sido adaptada como una obra que consiste en movimiento (p. ej., danza)."@es,
        "Expression d’une œuvre qui a été adaptée en œuvre consistant en mouvement (par exemple, de la danse)."@fr ;
    rdakit:toolkitLabel "choreographic adaptation of (expression)"@en,
        "adaptación coreográfica de (expresión)"@es,
        "adaptation chorégraphique de (expression)"@fr ;
    reg:hasSubproperty <http://rdaregistry.info/Elements/e/object/P20183> ;
    reg:hasUnconstrained <http://rdaregistry.info/Elements/u/P60293> ;
    reg:lexicalAlias <http://rdaregistry.info/Elements/e/choreographicAdaptationOfExpression.en> ;
    reg:name "choreographicAdaptationOfExpression"@en ;
    reg:status <http://metadataregistry.org/uri/RegStatus/1001> ;
    rdfs:domain <http://rdaregistry.info/Elements/c/C10006> ;
    rdfs:isDefinedBy <http://rdaregistry.info/Elements/e/> ;
    rdfs:subPropertyOf <http://rdaregistry.info/Elements/e/P20152> ;
    skos:definition "Relates an expression to an expression of a work that has been adapted as a work consisting of movement."@en .

<http://rdaregistry.info/Elements/e/P20184> a rdf:Property ;
    rdfs:label "is expanded version of (expression)"@en ;
    rdakit:instructionNumber "24.5" ;
    rdakit:toolkitDefinition "An expression of a work used as the basis for a derivative work that enlarges upon the content of a source work."@en,
        "Una expresión de una obra utilizada como base para una obra derivada que alarga el contenido de la obra fuente."@es,
        "Expression d’une œuvre servant de base à une œuvre dérivée qui accroît le contenu de l’œuvre source."@fr ;
    rdakit:toolkitLabel "expanded version of (expression)"@en,
        "versión ampliada de (expresión)"@es,
        "version augmentée de (expression)"@fr ;
    reg:hasSubproperty <http://rdaregistry.info/Elements/e/object/P20184> ;
    reg:hasUnconstrained <http://rdaregistry.info/Elements/u/P60294> ;
    reg:lexicalAlias <http://rdaregistry.info/Elements/e/expandedVersionOfExpression.en> ;
    reg:name "expandedVersionOfExpression"@en ;
    reg:status <http://metadataregistry.org/uri/RegStatus/1001> ;
    rdfs:domain <http://rdaregistry.info/Elements/c/C10006> ;
    rdfs:isDefinedBy <http://rdaregistry.info/Elements/e/> ;
    rdfs:subPropertyOf <http://rdaregistry.info/Elements/e/P20204> ;
    skos:definition "Relates an expression to an expression of a work used as the basis for a derivative work that enlarges upon the content of a source work."@en .

<http://rdaregistry.info/Elements/e/P20185> a rdf:Property ;
    rdfs:label "is remake of (expression)"@en ;
    rdakit:instructionNumber "24.5" ;
    rdakit:toolkitDefinition "An expression of a work used as a basis for a new motion picture, radio program, television program, or video."@en,
        "Una expresión de una obra utilizada como base para una nueva película cinematográfica, programa de radio, televisión o video."@es,
        "Expression d’une œuvre servant de base à un nouveau film, une nouvelle émission de radio, une nouvelle émission de télévision ou une nouvelle vidéo."@fr ;
    rdakit:toolkitLabel "remake of (expression)"@en,
        "remake de (expresión)"@es,
        "nouvelle version de (expression)"@fr ;
    reg:hasSubproperty <http://rdaregistry.info/Elements/e/object/P20185> ;
    reg:hasUnconstrained <http://rdaregistry.info/Elements/u/P60295> ;
    reg:lexicalAlias <http://rdaregistry.info/Elements/e/remakeOfExpression.en> ;
    reg:name "remakeOfExpression"@en ;
    reg:status <http://metadataregistry.org/uri/RegStatus/1001> ;
    rdfs:domain <http://rdaregistry.info/Elements/c/C10006> ;
    rdfs:isDefinedBy <http://rdaregistry.info/Elements/e/> ;
    rdfs:subPropertyOf <http://rdaregistry.info/Elements/e/P20204> ;
    skos:definition "Relates an expression to an expression of a work used as a basis for a new motion picture, radio program, television program, or video."@en .

<http://rdaregistry.info/Elements/e/P20186> a rdf:Property ;
    rdfs:label "is paraphrase of (expression)"@en ;
    rdakit:instructionNumber "24.5" ;
    rdakit:toolkitDefinition "An expression of a work used as the basis for a paraphrase, i.e., a restating of the content of a source work in a different form."@en,
        "Una expresión de una obra utilizada como base para una paráfrasis, i. e., replanteamiento del contenido de la obra fuente en una forma diferente."@es,
        "Expression d’une œuvre servant de base à une paraphrase, c’est-à-dire une reprise du contenu de l’œuvre source sous une formulation différente."@fr ;
    rdakit:toolkitLabel "paraphrase of (expression)"@en,
        "paráfrasis de (expresión)"@es,
        "paraphrase de (expression)"@fr ;
    reg:hasSubproperty <http://rdaregistry.info/Elements/e/object/P20186> ;
    reg:hasUnconstrained <http://rdaregistry.info/Elements/u/P60296> ;
    reg:lexicalAlias <http://rdaregistry.info/Elements/e/paraphraseOfExpression.en> ;
    reg:name "paraphraseOfExpression"@en ;
    reg:status <http://metadataregistry.org/uri/RegStatus/1001> ;
    rdfs:domain <http://rdaregistry.info/Elements/c/C10006> ;
    rdfs:isDefinedBy <http://rdaregistry.info/Elements/e/> ;
    rdfs:subPropertyOf <http://rdaregistry.info/Elements/e/P20204> ;
    skos:definition "Relates an expression to an expression of a work used as the basis for a paraphrase, i.e., a restating of the content of a source work in a different form."@en .

<http://rdaregistry.info/Elements/e/P20187> a rdf:Property ;
    reg:status <http://metadataregistry.org/uri/RegStatus/1008> ;
    rdfs:isDefinedBy <http://rdaregistry.info/Elements/e/> ;
    rdfs:subPropertyOf <http://rdaregistry.info/Elements/e/P20072> .

<http://rdaregistry.info/Elements/e/P20188> a rdf:Property ;
    rdfs:label "is index to (expression)"@en ;
    rdakit:instructionNumber "24.5" ;
    rdakit:toolkitDefinition "An expression of a work used as the basis for an index, i.e., a systematic, alphabetical guide to the contents of a predominant expression, usually keyed to page numbers or other reference codes."@en,
        "Una expresión de una obra utilizada como base para un índice, i.e., una guía alfabética y sistemática del contenido la entidad principal, generalmente indicando los números de página u otros códigos de referencia."@es,
        "Expression d’une œuvre servant de base à un index, c’est-à-dire un guide méthodique et alphabétique du contenu de l’expression prédominante, renvoyant généralement à des numéros de page ou à d’autres codes de référence."@fr ;
    rdakit:toolkitLabel "index to (expression)"@en,
        "índice de (expresión)"@es,
        "index de (expression)"@fr ;
    reg:hasSubproperty <http://rdaregistry.info/Elements/e/object/P20188> ;
    reg:hasUnconstrained <http://rdaregistry.info/Elements/u/P60302> ;
    reg:lexicalAlias <http://rdaregistry.info/Elements/e/indexToExpression.en> ;
    reg:name "indexToExpression"@en ;
    reg:status <http://metadataregistry.org/uri/RegStatus/1001> ;
    rdfs:domain <http://rdaregistry.info/Elements/c/C10006> ;
    rdfs:isDefinedBy <http://rdaregistry.info/Elements/e/> ;
    rdfs:subPropertyOf <http://rdaregistry.info/Elements/e/P20192> ;
    skos:definition "Relates an expression to an expression of a work used as the basis for an index, i.e., a systematic, alphabetical guide to the contents of a predominant expression, usually keyed to page numbers or other reference codes."@en .

<http://rdaregistry.info/Elements/e/P20189> a rdf:Property ;
    rdfs:label "is revision of"@en ;
    rdakit:instructionNumber "24.5" ;
    rdakit:toolkitDefinition "An expression of a work used as the basis for an updated, corrected, or expanded version."@en,
        "Una expresión de una obra utilizada como base para una versión actualizada, corregida o ampliada."@es,
        "Expression d’une œuvre servant de base à une version mise à jour, corrigée ou augmentée."@fr ;
    rdakit:toolkitLabel "revision of"@en,
        "revisión de"@es,
        "révision de"@fr ;
    reg:hasSubproperty <http://rdaregistry.info/Elements/e/object/P20189> ;
    reg:hasUnconstrained <http://rdaregistry.info/Elements/u/P60303> ;
    reg:lexicalAlias <http://rdaregistry.info/Elements/e/revisionOf.en> ;
    reg:name "revisionOf"@en ;
    reg:status <http://metadataregistry.org/uri/RegStatus/1001> ;
    rdfs:domain <http://rdaregistry.info/Elements/c/C10006> ;
    rdfs:isDefinedBy <http://rdaregistry.info/Elements/e/> ;
    rdfs:subPropertyOf <http://rdaregistry.info/Elements/e/P20204> ;
    skos:definition "Relates an expression to an expression of a work used as the basis for an updated, corrected, or expanded version."@en .

<http://rdaregistry.info/Elements/e/P20190> a rdf:Property ;
    rdfs:label "is libretto based on (expression)"@en ;
    rdakit:instructionNumber "24.5" ;
    rdakit:toolkitDefinition "An expression of a work used as the basis for the text of an opera or other work for the musical stage, or an oratorio."@en,
        "Una expresión de una obra usada como base para el texto de una ópera u otra obra para representación musical u oratorio."@es,
        "Expression d’une œuvre servant de base au texte d’un opéra ou d’une autre œuvre pour la scène musicale, ou bien d’un oratorio."@fr ;
    rdakit:toolkitLabel "libretto based on (expression)"@en,
        "libreto basado en (expresión)"@es,
        "livret basé sur (expression)"@fr ;
    reg:hasSubproperty <http://rdaregistry.info/Elements/e/object/P20190> ;
    reg:hasUnconstrained <http://rdaregistry.info/Elements/u/P60304> ;
    reg:lexicalAlias <http://rdaregistry.info/Elements/e/librettoBasedOnExpression.en> ;
    reg:name "librettoBasedOnExpression"@en ;
    reg:status <http://metadataregistry.org/uri/RegStatus/1001> ;
    rdfs:domain <http://rdaregistry.info/Elements/c/C10006> ;
    rdfs:isDefinedBy <http://rdaregistry.info/Elements/e/> ;
    rdfs:subPropertyOf <http://rdaregistry.info/Elements/e/P20152> ;
    skos:definition "Relates an expression to an expression of a work that has been adapted as the text of an opera or other work for the musical stage, or an oratorio."@en .

<http://rdaregistry.info/Elements/e/P20191> a rdf:Property ;
    rdfs:label "is continued by (expression)"@en ;
    rdakit:instructionNumber "24.5" ;
    rdakit:toolkitDefinition "An expression of a work whose content continues an expression of an earlier work."@en,
        "Una expresión de una obra cuyo contenido continúa una entidad anterior bajo un título nuevo."@es,
        "Expression d’une œuvre dont le contenu continue une expression d’une œuvre antérieure."@fr ;
    rdakit:toolkitLabel "continued by (expression)"@en,
        "continuada por (expresión)"@es,
        "continué par (expression)"@fr ;
    reg:hasSubproperty <http://rdaregistry.info/Elements/e/object/P20191> ;
    reg:hasUnconstrained <http://rdaregistry.info/Elements/u/P60306> ;
    reg:lexicalAlias <http://rdaregistry.info/Elements/e/continuedByExpression.en> ;
    reg:name "continuedByExpression"@en ;
    reg:status <http://metadataregistry.org/uri/RegStatus/1001> ;
    rdfs:domain <http://rdaregistry.info/Elements/c/C10006> ;
    rdfs:isDefinedBy <http://rdaregistry.info/Elements/e/> ;
    rdfs:subPropertyOf <http://rdaregistry.info/Elements/e/P20169> ;
    skos:definition "Relates an expression to an expression of a work whose content continues an expression of an earlier work."@en ;
    skos:scopeNote "This relationship applies generally to serials."@en .

<http://rdaregistry.info/Elements/e/P20193> a rdf:Property ;
    rdfs:label "is abstracts for (expression)"@en ;
    rdakit:instructionNumber "24.5" ;
    rdakit:toolkitDefinition "An expression of a work whose contents have been abstracted by an abstracting and indexing service."@en,
        "Una expresión de una obra cuyos contenidos han sido resumidos por un servicio de indización y resúmenes."@es,
        "Expression d’une œuvre dont le contenu a été résumé par un service d’analyse et d’indexation."@fr ;
    rdakit:toolkitLabel "abstracts for (expression)"@en,
        "resúmenes de (expresión)"@es,
        "résumés analytiques pour (expression)"@fr ;
    reg:hasSubproperty <http://rdaregistry.info/Elements/e/object/P20193> ;
    reg:hasUnconstrained <http://rdaregistry.info/Elements/u/P60308> ;
    reg:lexicalAlias <http://rdaregistry.info/Elements/e/abstractsForExpression.en> ;
    reg:name "abstractsForExpression"@en ;
    reg:status <http://metadataregistry.org/uri/RegStatus/1001> ;
    rdfs:domain <http://rdaregistry.info/Elements/c/C10006> ;
    rdfs:isDefinedBy <http://rdaregistry.info/Elements/e/> ;
    rdfs:subPropertyOf <http://rdaregistry.info/Elements/e/P20204> ;
    skos:definition "Relates an expression to an expression of a work whose contents have been abstracted by an abstracting and indexing service."@en .

<http://rdaregistry.info/Elements/e/P20194> a rdf:Property ;
    rdfs:label "is indexing for (expression)"@en ;
    rdakit:instructionNumber "24.5" ;
    rdakit:toolkitDefinition "An expression of a work whose contents have been indexed by an abstracting and indexing service."@en,
        "Una expresión de una obra cuyo contenido ha sido indizado por un servicio de indización y resúmenes."@es,
        "Expression d’une œuvre dont le contenu a été indexé par un service d’analyse et d’indexation."@fr ;
    rdakit:toolkitLabel "indexing for (expression)"@en,
        "indización de (expresión)"@es,
        "indexation pour (expression)"@fr ;
    reg:hasSubproperty <http://rdaregistry.info/Elements/e/object/P20194> ;
    reg:hasUnconstrained <http://rdaregistry.info/Elements/u/P60309> ;
    reg:lexicalAlias <http://rdaregistry.info/Elements/e/indexingForExpression.en> ;
    reg:name "indexingForExpression"@en ;
    reg:status <http://metadataregistry.org/uri/RegStatus/1001> ;
    rdfs:domain <http://rdaregistry.info/Elements/c/C10006> ;
    rdfs:isDefinedBy <http://rdaregistry.info/Elements/e/> ;
    rdfs:subPropertyOf <http://rdaregistry.info/Elements/e/P20204> ;
    skos:definition "Relates an expression to an expression of a work whose contents have been indexed by an abstracting and indexing service."@en .

<http://rdaregistry.info/Elements/e/P20196> a rdf:Property ;
    rdfs:label "is parody of (expression)"@en ;
    rdakit:instructionNumber "24.5" ;
    rdakit:toolkitDefinition "An expression of a work whose style or content is imitated for comic effect."@en,
        "Una expresión de una obra cuyo estilo o contenido es imitado para crear un efecto cómico."@es,
        "Expression d’une œuvre dont le style ou le contenu est imité dans le but de produire un effet comique."@fr ;
    rdakit:toolkitLabel "parody of (expression)"@en,
        "parodia de (expresión)"@es,
        "parodie de (expression)"@fr ;
    reg:hasSubproperty <http://rdaregistry.info/Elements/e/object/P20196> ;
    reg:hasUnconstrained <http://rdaregistry.info/Elements/u/P60312> ;
    reg:lexicalAlias <http://rdaregistry.info/Elements/e/parodyOfExpression.en> ;
    reg:name "parodyOfExpression"@en ;
    reg:status <http://metadataregistry.org/uri/RegStatus/1001> ;
    rdfs:domain <http://rdaregistry.info/Elements/c/C10006> ;
    rdfs:isDefinedBy <http://rdaregistry.info/Elements/e/> ;
    rdfs:subPropertyOf <http://rdaregistry.info/Elements/e/P20195> ;
    skos:definition "Relates an expression to an expression of a work whose style or content is imitated for comic effect."@en .

<http://rdaregistry.info/Elements/e/P20197> a rdf:Property ;
    rdfs:label "is finding aid for (expression)"@en ;
    rdakit:instructionNumber "24.5" ;
    rdakit:toolkitDefinition "An expression of an archival collection that is described in a finding aid, i.e., a guide to the organization, arrangement, and contents of the collection."@en,
        "Una expresión de una colección archivística que está descrita en una guía de búsqueda, i.e., una guía para la organización, ordenación y contenido de la colección."@es,
        "Expression d’une collection ou d’un fonds d’archives qui est décrit dans un instrument de recherche, c’est-à-dire un guide de l’organisation, du classement et du contenu de la collection ou du fonds."@fr ;
    rdakit:toolkitLabel "finding aid for (expression)"@en,
        "guía de búsqueda de (expresión)"@es,
        "instrument de recherche pour (expression)"@fr ;
    reg:hasSubproperty <http://rdaregistry.info/Elements/e/object/P20197> ;
    reg:hasUnconstrained <http://rdaregistry.info/Elements/u/P60474> ;
    reg:lexicalAlias <http://rdaregistry.info/Elements/e/findingAidForExpression.en> ;
    reg:name "findingAidForExpression"@en ;
    reg:status <http://metadataregistry.org/uri/RegStatus/1001> ;
    rdfs:domain <http://rdaregistry.info/Elements/c/C10006> ;
    rdfs:isDefinedBy <http://rdaregistry.info/Elements/e/> ;
    rdfs:subPropertyOf <http://rdaregistry.info/Elements/e/P20192> ;
    skos:definition "Relates an expression to an expression of an archival collection that is described in a finding aid, i.e., a guide to the organization, arrangement, and contents of the collection."@en .

<http://rdaregistry.info/Elements/e/P20198> a rdf:Property ;
    rdfs:label "is replacement in part of (expression)"@en ;
    rdakit:instructionNumber "24.5" ;
    rdakit:toolkitDefinition "An expression of an earlier work whose content has been partially replaced by a later expression, usually because the later work contains updated or new information that makes the earlier expression obsolete."@en,
        "Una expresión de una obra anterior cuyo contenido ha sido reemplazado parcialmente por una expresión posterior, generalmente porque la obra posterior contiene información actualizada o nueva que hace obsoleta la expresión anterior."@es,
        "Expression d’une œuvre antérieure dont le contenu a été partiellement remplacé par une expression ultérieure, généralement parce que l’œuvre ultérieure contient de l’information nouvelle ou mise à jour qui rend l’expression antérieure obsolète."@fr ;
    rdakit:toolkitLabel "replacement in part of (expression)"@en,
        "reemplazo en parte de (expresión)"@es,
        "remplacement partiel de (expression)"@fr ;
    reg:hasSubproperty <http://rdaregistry.info/Elements/e/object/P20198> ;
    reg:hasUnconstrained <http://rdaregistry.info/Elements/u/P60479> ;
    reg:lexicalAlias <http://rdaregistry.info/Elements/e/replacementInPartOfExpression.en> ;
    reg:name "replacementInPartOfExpression"@en ;
    reg:status <http://metadataregistry.org/uri/RegStatus/1001> ;
    rdfs:domain <http://rdaregistry.info/Elements/c/C10006> ;
    rdfs:isDefinedBy <http://rdaregistry.info/Elements/e/> ;
    rdfs:subPropertyOf <http://rdaregistry.info/Elements/e/P20154> ;
    skos:definition "Relates an expression to an expression of an earlier work whose content has been partially replaced by a later expression, usually because the later work contains updated or new information that makes the earlier expression obsolete."@en ;
    skos:scopeNote "This relationship applies generally to single-part units, multipart monographs, and integrating resources."@en .

<http://rdaregistry.info/Elements/e/P20199> a rdf:Property ;
    rdfs:label "is replacement of (expression)"@en ;
    rdakit:instructionNumber "24.5" ;
    rdakit:toolkitDefinition "An expression of an earlier work whose content has been replaced by a later expression, usually because the later work contains updated or new information that makes the earlier expression obsolete."@en,
        "Una expresión de una obra anterior cuyo contenido ha sido reemplazado por una expresión posterior, generalmente porque la obra posterior contiene información actualizada o nueva que hace obsoleta la expresión anterior."@es,
        "Expression d’une œuvre antérieure dont le contenu a été remplacé par une expression ultérieure, généralement parce que l’œuvre ultérieure contient de l’information nouvelle ou mise à jour qui rend l’expression antérieure obsolète."@fr ;
    rdakit:toolkitLabel "replacement of (expression)"@en,
        "reemplazo de (expresión)"@es,
        "remplacement de (expression)"@fr ;
    reg:hasSubproperty <http://rdaregistry.info/Elements/e/object/P20199> ;
    reg:hasUnconstrained <http://rdaregistry.info/Elements/u/P60480> ;
    reg:lexicalAlias <http://rdaregistry.info/Elements/e/replacementOfExpression.en> ;
    reg:name "replacementOfExpression"@en ;
    reg:status <http://metadataregistry.org/uri/RegStatus/1001> ;
    rdfs:domain <http://rdaregistry.info/Elements/c/C10006> ;
    rdfs:isDefinedBy <http://rdaregistry.info/Elements/e/> ;
    rdfs:subPropertyOf <http://rdaregistry.info/Elements/e/P20154> ;
    skos:definition "Relates an expression to an expression of an earlier work whose content has been replaced by a later expression, usually because the later work contains updated or new information that makes the earlier expression obsolete."@en ;
    skos:scopeNote "This relationship applies generally to single-part units, multipart monographs, and integrating resources."@en .

<http://rdaregistry.info/Elements/e/P20200> a rdf:Property ;
    rdfs:label "is split into (expression)"@en ;
    rdakit:instructionNumber "24.5" ;
    rdakit:toolkitDefinition "An expression of one of two or more works resulting from division of an earlier expression into separate expressions."@en,
        "Una expresión de una de dos o más obras que resulta de la división de una entidad anterior en entidades separadas."@es,
        "Expression de l’une de deux ou plusieurs œuvres résultant de la division d’une expression antérieure en expressions séparées."@fr ;
    rdakit:toolkitLabel "split into (expression)"@en,
        "escindida en (expresión)"@es,
        "scindé en (expression)"@fr ;
    reg:hasSubproperty <http://rdaregistry.info/Elements/e/object/P20200> ;
    reg:hasUnconstrained <http://rdaregistry.info/Elements/u/P60503> ;
    reg:lexicalAlias <http://rdaregistry.info/Elements/e/splitIntoExpression.en> ;
    reg:name "splitIntoExpression"@en ;
    reg:status <http://metadataregistry.org/uri/RegStatus/1001> ;
    rdfs:domain <http://rdaregistry.info/Elements/c/C10006> ;
    rdfs:isDefinedBy <http://rdaregistry.info/Elements/e/> ;
    rdfs:subPropertyOf <http://rdaregistry.info/Elements/e/P20169> ;
    skos:definition "Relates an expression to an expression of one of two or more works resulting from division of an earlier expression into separate expressions."@en .

<http://rdaregistry.info/Elements/e/P20201> a rdf:Property ;
    rdfs:label "is merger of (expression)"@en ;
    rdakit:instructionNumber "24.5" ;
    rdakit:toolkitDefinition "An expression of a work that came together with one or more other expressions to form a new expression."@en,
        "Una expresión de una obra que se une con una o más expresiones para formar una expresión nueva."@es,
        "Expression d’une œuvre qui s’est assemblée avec une ou plusieurs autres expressions pour former la nouvelle expression."@fr ;
    rdakit:toolkitLabel "merger of (expression)"@en,
        "fusión de (expresión)"@es,
        "fusion de (expression)"@fr ;
    reg:hasSubproperty <http://rdaregistry.info/Elements/e/object/P20201> ;
    reg:hasUnconstrained <http://rdaregistry.info/Elements/u/P60505> ;
    reg:lexicalAlias <http://rdaregistry.info/Elements/e/mergerOfExpression.en> ;
    reg:name "mergerOfExpression"@en ;
    reg:status <http://metadataregistry.org/uri/RegStatus/1001> ;
    rdfs:domain <http://rdaregistry.info/Elements/c/C10006> ;
    rdfs:isDefinedBy <http://rdaregistry.info/Elements/e/> ;
    rdfs:subPropertyOf <http://rdaregistry.info/Elements/e/P20154> ;
    skos:definition "Relates an expression to an expression of a work that came together with one or more other expressions to form a new expression."@en .

<http://rdaregistry.info/Elements/e/P20211> a rdf:Property ;
    rdfs:label "is revised as"@en ;
    rdakit:instructionNumber "24.5" ;
    rdakit:toolkitDefinition "An expression of a work that has been updated, corrected, or expanded."@en,
        "Una expresión de una obra que fue actualizada, corregida o ampliada."@es,
        "Expression d’une œuvre qui a été mise à jour, corrigée ou augmentée."@fr ;
    rdakit:toolkitLabel "revised as"@en,
        "revisada como"@es,
        "révisé comme"@fr ;
    reg:hasSubproperty <http://rdaregistry.info/Elements/e/object/P20211> ;
    reg:hasUnconstrained <http://rdaregistry.info/Elements/u/P60245> ;
    reg:lexicalAlias <http://rdaregistry.info/Elements/e/revisedAs.en> ;
    reg:name "revisedAs"@en ;
    reg:status <http://metadataregistry.org/uri/RegStatus/1001> ;
    rdfs:domain <http://rdaregistry.info/Elements/c/C10006> ;
    rdfs:isDefinedBy <http://rdaregistry.info/Elements/e/> ;
    rdfs:subPropertyOf <http://rdaregistry.info/Elements/e/P20203> ;
    skos:definition "Relates an expression to an expression of a work that has been updated, corrected, or expanded."@en .

<http://rdaregistry.info/Elements/e/P20212> a rdf:Property ;
    rdfs:label "is merged to form (expression)"@en ;
    rdakit:instructionNumber "24.5" ;
    rdakit:toolkitDefinition "An expression of a work formed from the coming together of two or more expressions."@en,
        "Una expresión de una obra formada de la unión de dos o más expresiones."@es,
        "Expression d’une œuvre formée par l’assemblage de deux ou plusieurs expressions."@fr ;
    rdakit:toolkitLabel "merged to form (expression)"@en,
        "fusionada para formar (expresión)"@es,
        "fusionné pour former (expression)"@fr ;
    reg:hasSubproperty <http://rdaregistry.info/Elements/e/object/P20212> ;
    reg:hasUnconstrained <http://rdaregistry.info/Elements/u/P60504> ;
    reg:lexicalAlias <http://rdaregistry.info/Elements/e/mergedToFormExpression.en> ;
    reg:name "mergedToFormExpression"@en ;
    reg:status <http://metadataregistry.org/uri/RegStatus/1001> ;
    rdfs:domain <http://rdaregistry.info/Elements/c/C10006> ;
    rdfs:isDefinedBy <http://rdaregistry.info/Elements/e/> ;
    rdfs:subPropertyOf <http://rdaregistry.info/Elements/e/P20169> ;
    skos:definition "Relates an expression to an expression of a work formed from the coming together of two or more expressions."@en .

<http://rdaregistry.info/Elements/e/P20213> a rdf:Property ;
    rdfs:label "has additional scale information"@en,
        "har övrig skalinformation"@sv ;
    rdakit:instructionNumber "7.25.5" ;
    rdakit:toolkitDefinition "An indication of supplemental information about scale."@en,
        "Información complementaria sobre la escala tal como una mención de medidas comparativas o la limitación de la escala a partes particulares del contenido de un recurso."@es,
        "Information complémentaire relative à l’échelle, comme un relevé de mesures comparatives ou une limitation de l’échelle à certaines portions du contenu."@fr ;
    rdakit:toolkitLabel "additional scale information"@en,
        "información adicional de la escala"@es,
        "information supplémentaire sur l’échelle"@fr,
        "övrig skalinformation"@sv ;
    reg:hasUnconstrained <http://rdaregistry.info/Elements/u/P60510> ;
    reg:lexicalAlias <http://rdaregistry.info/Elements/e/additionalScaleInformation.en> ;
    reg:name "additionalScaleInformation"@en ;
    reg:status <http://metadataregistry.org/uri/RegStatus/1001> ;
    rdfs:domain <http://rdaregistry.info/Elements/c/C10006> ;
    rdfs:isDefinedBy <http://rdaregistry.info/Elements/e/> ;
    rdfs:subPropertyOf <http://rdaregistry.info/Elements/e/P20228> ;
    skos:definition "Relates an expression to an indication of supplemental information about scale."@en ;
    skos:scopeNote "Additional scale information includes statement of comparative measurements or limitation of the scale to particular parts of the content of an expression."@en .

<http://rdaregistry.info/Elements/e/P20220> a rdf:Property ;
    reg:status <http://metadataregistry.org/uri/RegStatus/1008> ;
    rdfs:isDefinedBy <http://rdaregistry.info/Elements/e/> ;
    rdfs:subPropertyOf <http://rdaregistry.info/Elements/e/P20224> .

<http://rdaregistry.info/Elements/e/P20221> a rdf:Property ;
    reg:status <http://metadataregistry.org/uri/RegStatus/1008> ;
    rdfs:isDefinedBy <http://rdaregistry.info/Elements/e/> ;
    rdfs:subPropertyOf <http://rdaregistry.info/Elements/e/P20224> .

<http://rdaregistry.info/Elements/e/P20222> a rdf:Property ;
    reg:status <http://metadataregistry.org/uri/RegStatus/1008> ;
    rdfs:isDefinedBy <http://rdaregistry.info/Elements/e/> ;
    rdfs:subPropertyOf <http://rdaregistry.info/Elements/e/P20224> .

<http://rdaregistry.info/Elements/e/P20223> a rdf:Property ;
    reg:status <http://metadataregistry.org/uri/RegStatus/1008> ;
    rdfs:isDefinedBy <http://rdaregistry.info/Elements/e/> ;
    rdfs:subPropertyOf <http://rdaregistry.info/Elements/e/P20224> .

<http://rdaregistry.info/Elements/e/P20226> a rdf:Property ;
    rdfs:label "has horizontal scale of cartographic content"@en ;
    rdakit:instructionNumber "7.25.3" ;
    rdakit:toolkitDefinition "A ratio of horizontal distances in cartographic content of an expression to the actual distances they represent."@en,
        "La proporción de las distancias horizontales en el contenido cartográfico de un recurso con las distancias reales que representan."@es,
        "Le rapport entre les distances horizontales dans le contenu cartographique d’une ressource et les distances réelles qu’elles représentent."@fr ;
    rdakit:toolkitLabel "horizontal scale of cartographic content"@en,
        "escala horizontal del contenido cartográfico"@es,
        "échelle des longueurs d’un contenu cartographique"@fr ;
    reg:hasUnconstrained <http://rdaregistry.info/Elements/u/P60563> ;
    reg:lexicalAlias <http://rdaregistry.info/Elements/e/horizontalScaleOfCartographicContent.en> ;
    reg:name "horizontalScaleOfCartographicContent"@en ;
    reg:status <http://metadataregistry.org/uri/RegStatus/1001> ;
    rdfs:domain <http://rdaregistry.info/Elements/c/C10006> ;
    rdfs:isDefinedBy <http://rdaregistry.info/Elements/e/> ;
    rdfs:subPropertyOf <http://rdaregistry.info/Elements/e/P20228> ;
    skos:definition "Relates an expression to a ratio of horizontal distances in cartographic content of an expression to the actual distances they represent."@en .

<http://rdaregistry.info/Elements/e/P20227> a rdf:Property ;
    rdfs:label "has scale of still image or three-dimensional form"@en,
        "har skala för stillbild eller tredimensionell bild"@sv ;
    rdakit:instructionNumber "7.25.2" ;
    rdakit:toolkitDefinition "A ratio of the dimensions of a still image or three-dimensional form contained or embodied in an expression to the dimensions of the thing that is represented."@en,
        "La proporción de las dimensiones de una imagen fija o forma tridimensional que está contenida o incorporada en un recurso con las dimensiones de la entidad que representa."@es,
        "Le rapport entre les dimensions d’une image fixe ou d’une forme tridimensionnelle, contenue ou matérialisée dans une ressource, et les dimensions de l’entité qu’elle représente."@fr ;
    rdakit:toolkitLabel "scale of still image or three-dimensional form"@en,
        "escala de una imagen fija o una forma tridimensional"@es,
        "échelle d’une image fixe ou d’une forme tridimensionnelle"@fr,
        "skala för stillbild eller tredimensionell bild"@sv ;
    reg:hasUnconstrained <http://rdaregistry.info/Elements/u/P60564> ;
    reg:lexicalAlias <http://rdaregistry.info/Elements/e/scaleOfStillImageOrThreeDimensionalForm.en> ;
    reg:name "scaleOfStillImageOrThreeDimensionalForm"@en ;
    reg:status <http://metadataregistry.org/uri/RegStatus/1001> ;
    rdfs:domain <http://rdaregistry.info/Elements/c/C10006> ;
    rdfs:isDefinedBy <http://rdaregistry.info/Elements/e/> ;
    rdfs:subPropertyOf <http://rdaregistry.info/Elements/e/P20228> ;
    skos:definition "Relates an expression to a ratio of the dimensions of a still image or three-dimensional form contained or embodied in an expression to the dimensions of the thing that is represented."@en .

<http://rdaregistry.info/Elements/e/P20230> a rdf:Property ;
    rdfs:label "has vertical scale of cartographic content"@en,
        "har vertikal skala för kartografiskt innehåll"@sv ;
    rdakit:instructionNumber "7.25.4" ;
    rdakit:toolkitDefinition "A scale of elevation or vertical dimension of cartographic content of an expression."@en,
        "La escala de elevación o dimensión vertical del contenido cartográfico de un recurso."@es,
        "L’échelle de l’élévation ou de la dimension verticale du contenu cartographique d’une ressource."@fr ;
    rdakit:toolkitLabel "vertical scale of cartographic content"@en,
        "escala vertical del contenido cartográfico"@es,
        "échelle des hauteurs d’un contenu cartographique"@fr,
        "vertikal skala för kartografiskt innehåll"@sv ;
    reg:hasUnconstrained <http://rdaregistry.info/Elements/u/P60579> ;
    reg:lexicalAlias <http://rdaregistry.info/Elements/e/verticalScaleOfCartographicContent.en> ;
    reg:name "verticalScaleOfCartographicContent"@en ;
    reg:status <http://metadataregistry.org/uri/RegStatus/1001> ;
    rdfs:domain <http://rdaregistry.info/Elements/c/C10006> ;
    rdfs:isDefinedBy <http://rdaregistry.info/Elements/e/> ;
    rdfs:subPropertyOf <http://rdaregistry.info/Elements/e/P20228> ;
    skos:definition "Relates an expression to a scale of elevation or vertical dimension of cartographic content of an expression."@en .

<http://rdaregistry.info/Elements/e/P20253> a rdf:Property ;
    rdfs:label "is choreography (expression)"@en ;
    rdakit:instructionNumber "24.5" ;
    rdakit:toolkitDefinition "An expression of a work that provides choreography for use in a related expression."@en,
        "Una expresión de una obra que proporciona la coreografía para uso en la expresión relacionada."@es,
        "Expression d’une œuvre qui fournit la chorégraphie destinée à être utilisée dans l’expression en relation."@fr ;
    rdakit:toolkitLabel "choreography (expression)"@en,
        "coreografía (expresión)"@es,
        "chorégraphie (expression)"@fr ;
    reg:hasSubproperty <http://rdaregistry.info/Elements/e/object/P20253> ;
    reg:hasUnconstrained <http://rdaregistry.info/Elements/u/P60740> ;
    reg:lexicalAlias <http://rdaregistry.info/Elements/e/choreographyExpression.en> ;
    reg:name "choreographyExpression"@en ;
    reg:status <http://metadataregistry.org/uri/RegStatus/1001> ;
    rdfs:domain <http://rdaregistry.info/Elements/c/C10006> ;
    rdfs:isDefinedBy <http://rdaregistry.info/Elements/e/> ;
    rdfs:subPropertyOf <http://rdaregistry.info/Elements/e/P20100> ;
    skos:definition "Relates an expression to an expression of a work that provides choreography for use in a related expression."@en .

<http://rdaregistry.info/Elements/e/P20254> a rdf:Property ;
    rdfs:label "is choreography for (expression)"@en ;
    rdakit:instructionNumber "24.5" ;
    rdakit:toolkitDefinition "An expression of a work that uses choreography of a related expression."@en,
        "Una expresión de una obra que usa la coreografía de la expresión relacionada."@es,
        "Expression d’une œuvre qui utilise la chorégraphie de l’expression en relation."@fr ;
    rdakit:toolkitLabel "choreography for (expression)"@en,
        "coreografía para (expresión)"@es,
        "chorégraphie pour (expression)"@fr ;
    reg:hasSubproperty <http://rdaregistry.info/Elements/e/object/P20254> ;
    reg:hasUnconstrained <http://rdaregistry.info/Elements/u/P60741> ;
    reg:lexicalAlias <http://rdaregistry.info/Elements/e/choreographyForExpression.en> ;
    reg:name "choreographyForExpression"@en ;
    reg:status <http://metadataregistry.org/uri/RegStatus/1001> ;
    rdfs:domain <http://rdaregistry.info/Elements/c/C10006> ;
    rdfs:isDefinedBy <http://rdaregistry.info/Elements/e/> ;
    rdfs:subPropertyOf <http://rdaregistry.info/Elements/e/P20100> ;
    skos:definition "Relates an expression to an expression of a work that uses choreography of a related expression."@en .

<http://rdaregistry.info/Elements/e/P20255> a rdf:Property ;
    rdfs:label "is adapted as graphic novel (expression)"@en ;
    rdakit:instructionNumber "24.5" ;
    rdakit:toolkitDefinition "A graphic novel based on a source expression."@en,
        "Una novela gráfica basada en la expresión fuente."@es,
        "Roman graphique basé sur l’expression source."@fr ;
    rdakit:toolkitLabel "adapted as graphic novel (expression)"@en,
        "adaptada como novela gráfica (expresión)"@es,
        "adapté en roman graphique (expression)"@fr ;
    reg:hasSubproperty <http://rdaregistry.info/Elements/e/object/P20255> ;
    reg:hasUnconstrained <http://rdaregistry.info/Elements/u/P60742> ;
    reg:lexicalAlias <http://rdaregistry.info/Elements/e/adaptedAsGraphicNovelExpression.en> ;
    reg:name "adaptedAsGraphicNovelExpression"@en ;
    reg:status <http://metadataregistry.org/uri/RegStatus/1001> ;
    rdfs:domain <http://rdaregistry.info/Elements/c/C10006> ;
    rdfs:isDefinedBy <http://rdaregistry.info/Elements/e/> ;
    rdfs:subPropertyOf <http://rdaregistry.info/Elements/e/P20153> ;
    skos:definition "Relates an expression to a graphic novel based on a source expression."@en .

<http://rdaregistry.info/Elements/e/P20256> a rdf:Property ;
    rdfs:label "is graphic novelization of (expression)"@en ;
    rdakit:instructionNumber "24.5" ;
    rdakit:toolkitDefinition "An expression of a work that has been adapted as a graphic novel."@en,
        "Una expresión de una obra que ha sido adaptada como una novela gráfica."@es,
        "Expression d’une œuvre qui a été adaptée en roman graphique."@fr ;
    rdakit:toolkitLabel "graphic novelization of (expression)"@en,
        "novelización gráfica de (expresión)"@es,
        "adaptation en roman graphique de (expression)"@fr ;
    reg:hasSubproperty <http://rdaregistry.info/Elements/e/object/P20256> ;
    reg:hasUnconstrained <http://rdaregistry.info/Elements/u/P60743> ;
    reg:lexicalAlias <http://rdaregistry.info/Elements/e/graphicNovelizationOfExpression.en> ;
    reg:name "graphicNovelizationOfExpression"@en ;
    reg:status <http://metadataregistry.org/uri/RegStatus/1001> ;
    rdfs:domain <http://rdaregistry.info/Elements/c/C10006> ;
    rdfs:isDefinedBy <http://rdaregistry.info/Elements/e/> ;
    rdfs:subPropertyOf <http://rdaregistry.info/Elements/e/P20152> ;
    skos:definition "Relates an expression to an expression of a work that has been adapted as a graphic novel."@en .

<http://rdaregistry.info/Elements/e/P20257> a rdf:Property ;
    rdfs:label "has visual effects provider"@en ;
    rdakit:instructionNumber "18.5" ;
    rdakit:toolkitDefinition "An agent contributing to an expression of a moving image work by designing and creating post-production visual effects."@en,
        "Una persona, familia o entidad corporativa que contribuye a una expresión de una obra de imagen en movimiento desarrollando y creando efectos visuales de post-producción."@es,
        "Personne, famille ou collectivité contribuant à une expression d’une œuvre d’images animées en concevant et en créant des effets visuels en postproduction."@fr ;
    rdakit:toolkitLabel "visual effects provider"@en,
        "productor de efectos visuales"@es,
        "fournisseur d’effets visuels"@fr ;
    reg:hasSubproperty <http://rdaregistry.info/Elements/e/object/P20257> ;
    reg:hasUnconstrained <http://rdaregistry.info/Elements/u/P60748> ;
    reg:lexicalAlias <http://rdaregistry.info/Elements/e/visualEffectsProvider.en> ;
    reg:name "visualEffectsProvider"@en ;
    reg:status <http://metadataregistry.org/uri/RegStatus/1001> ;
    rdfs:domain <http://rdaregistry.info/Elements/c/C10006> ;
    rdfs:isDefinedBy <http://rdaregistry.info/Elements/e/> ;
    rdfs:subPropertyOf <http://rdaregistry.info/Elements/e/P20053> ;
    skos:definition "Relates an expression to an agent contributing to an expression of a moving image work by designing and creating post-production visual effects."@en .

<http://rdaregistry.info/Elements/e/P20258> a rdf:Property ;
    rdfs:label "has special effects provider"@en ;
    rdakit:instructionNumber "18.5" ;
    rdakit:toolkitDefinition "An agent contributing to an expression of a moving image or audio work by designing and creating on-set special effects such as on-set mechanical effects and in-camera optical effects."@en,
        "Una persona, familia o entidad corporativa que contribuye a una expresión de una imagen en movimiento u obra sonora mediante el diseño y creación de efectos especiales del set (efectos mecánicos en el set y efectos ópticos en cámara)."@es,
        "Personne, famille ou collectivité contribuant à une expression d’une œuvre d’images animées ou d’une œuvre audio en concevant et en créant des effets spéciaux de plateau (effets mécaniques de plateau et effets d’optique dans la caméra)."@fr ;
    rdakit:toolkitLabel "special effects provider"@en,
        "productor de efectos especiales"@es,
        "fournisseur d’effets spéciaux"@fr ;
    reg:hasSubproperty <http://rdaregistry.info/Elements/e/object/P20258> ;
    reg:hasUnconstrained <http://rdaregistry.info/Elements/u/P60749> ;
    reg:lexicalAlias <http://rdaregistry.info/Elements/e/specialEffectsProvider.en> ;
    reg:name "specialEffectsProvider"@en ;
    reg:status <http://metadataregistry.org/uri/RegStatus/1001> ;
    rdfs:domain <http://rdaregistry.info/Elements/c/C10006> ;
    rdfs:isDefinedBy <http://rdaregistry.info/Elements/e/> ;
    rdfs:subPropertyOf <http://rdaregistry.info/Elements/e/P20053> ;
    skos:definition "Relates an expression to an agent contributing to an expression of a moving image or audio work by designing and creating on-set special effects such as on-set mechanical effects and in-camera optical effects."@en .

<http://rdaregistry.info/Elements/e/P20259> a rdf:Property ;
    rdfs:label "has letterer"@en ;
    rdakit:instructionNumber "18.5" ;
    rdakit:toolkitDefinition "An illustrator contributing to an expression of a comic book, graphic novel, etc., by drawing the text and graphic sound effects."@en,
        "Un ilustrador que contribuye a una expresión de un libro cómico, novela gráfica, etc., mediante el dibujo del texto y efectos de sonido gráfico."@es,
        "Illustrateur contribuant à une expression d’une bande dessinée, d’un roman graphique, etc. en dessinant le texte et les effets sonores graphiques."@fr ;
    rdakit:toolkitLabel "letterer"@en,
        "rotulista"@es,
        "lettreur"@fr ;
    reg:hasSubproperty <http://rdaregistry.info/Elements/e/object/P20259> ;
    reg:hasUnconstrained <http://rdaregistry.info/Elements/u/P60750> ;
    reg:lexicalAlias <http://rdaregistry.info/Elements/e/letterer.en> ;
    reg:name "letterer"@en ;
    reg:status <http://metadataregistry.org/uri/RegStatus/1001> ;
    rdfs:domain <http://rdaregistry.info/Elements/c/C10006> ;
    rdfs:isDefinedBy <http://rdaregistry.info/Elements/e/> ;
    rdfs:subPropertyOf <http://rdaregistry.info/Elements/e/P20051> ;
    skos:definition "Relates an expression to an illustrator contributing to an expression of a comic book, graphic novel, etc., by drawing the text and graphic sound effects."@en .

<http://rdaregistry.info/Elements/e/P20268> a rdf:Property ;
    rdfs:label "is subject of (expression)"@en ;
    rdakit:toolkitDefinition "A work that is about an expression."@en,
        "Una obra que trata sobre la expresión."@es ;
    rdakit:toolkitLabel "subject of (expression)"@en,
        "materia de (expresión)"@es ;
    reg:hasSubproperty <http://rdaregistry.info/Elements/e/P20269>,
        <http://rdaregistry.info/Elements/e/object/P20268> ;
    reg:hasUnconstrained <http://rdaregistry.info/Elements/u/P60806> ;
    reg:lexicalAlias <http://rdaregistry.info/Elements/e/subjectOfExpression.en> ;
    reg:name "subjectOfExpression"@en ;
    reg:status <http://metadataregistry.org/uri/RegStatus/1001> ;
    rdfs:domain <http://rdaregistry.info/Elements/c/C10006> ;
    rdfs:isDefinedBy <http://rdaregistry.info/Elements/e/> ;
    rdfs:subPropertyOf <http://rdaregistry.info/Elements/w/P10283> ;
    skos:definition "Relates an expression to a work that is about an expression."@en .

<http://rdaregistry.info/Elements/e/P20270> a rdf:Property ;
    rdfs:label "is analysed in (expression)"@en ;
    rdakit:instructionNumber "23.5" ;
    rdakit:toolkitDefinition "A work that examines a source expression to identify its components and their relations."@en,
        "Una obra que examina la expresión fuente para identificar sus componentes y sus relaciones."@es,
        "Expression d’une œuvre qui examine l’expression source pour identifier ses composantes et leurs relations."@fr ;
    rdakit:toolkitLabel "analysed in (expression)"@en,
        "analizada en (expresión)"@es,
        "analysé dans (expression)"@fr ;
    reg:hasSubproperty <http://rdaregistry.info/Elements/e/object/P20270> ;
    reg:hasUnconstrained <http://rdaregistry.info/Elements/u/P60219> ;
    reg:lexicalAlias <http://rdaregistry.info/Elements/e/analysedInExpression.en> ;
    reg:name "analysedInExpression"@en ;
    reg:status <http://metadataregistry.org/uri/RegStatus/1001> ;
    rdfs:domain <http://rdaregistry.info/Elements/c/C10006> ;
    rdfs:isDefinedBy <http://rdaregistry.info/Elements/e/> ;
    rdfs:subPropertyOf <http://rdaregistry.info/Elements/e/P20269> ;
    skos:definition "Relates an expression to a work that examines a source expression to identify its components and their relations."@en .

<http://rdaregistry.info/Elements/e/P20271> a rdf:Property ;
    rdfs:label "is commentary in (expression)"@en ;
    rdakit:instructionNumber "23.5" ;
    rdakit:toolkitDefinition "A work that contains a set of explanatory or critical notes on a described expression."@en,
        "Una obra que contiene un conjunto de notas críticas o explicativas de la expresión descrita."@es,
        "Expression d’une œuvre qui contient un ensemble de notes explicatives ou critiques sur l’expression décrite."@fr ;
    rdakit:toolkitLabel "commentary in (expression)"@en,
        "comentario en (expresión)"@es,
        "commentaire dans (expression)"@fr ;
    reg:hasSubproperty <http://rdaregistry.info/Elements/e/object/P20271> ;
    reg:hasUnconstrained <http://rdaregistry.info/Elements/u/P60213> ;
    reg:lexicalAlias <http://rdaregistry.info/Elements/e/commentaryInExpression.en> ;
    reg:name "commentaryInExpression"@en ;
    reg:status <http://metadataregistry.org/uri/RegStatus/1001> ;
    rdfs:domain <http://rdaregistry.info/Elements/c/C10006> ;
    rdfs:isDefinedBy <http://rdaregistry.info/Elements/e/> ;
    rdfs:subPropertyOf <http://rdaregistry.info/Elements/e/P20269> ;
    skos:definition "Relates an expression to a work that contains a set of explanatory or critical notes on a described expression."@en .

<http://rdaregistry.info/Elements/e/P20272> a rdf:Property ;
    rdfs:label "is critiqued in (expression)"@en ;
    rdakit:instructionNumber "23.5" ;
    rdakit:toolkitDefinition "A work that contains a critical evaluation of a described expression."@en,
        "Una obra que contiene una evaluación crítica de la expresión descrita."@es,
        "Expression d’une œuvre qui contient une évaluation critique de l’expression décrite."@fr ;
    rdakit:toolkitLabel "critiqued in (expression)"@en,
        "criticada en (expresión)"@es,
        "critiqué dans (expression)"@fr ;
    reg:hasSubproperty <http://rdaregistry.info/Elements/e/object/P20272> ;
    reg:hasUnconstrained <http://rdaregistry.info/Elements/u/P60212> ;
    reg:lexicalAlias <http://rdaregistry.info/Elements/e/critiquedInExpression.en> ;
    reg:name "critiquedInExpression"@en ;
    reg:status <http://metadataregistry.org/uri/RegStatus/1001> ;
    rdfs:domain <http://rdaregistry.info/Elements/c/C10006> ;
    rdfs:isDefinedBy <http://rdaregistry.info/Elements/e/> ;
    rdfs:subPropertyOf <http://rdaregistry.info/Elements/e/P20269> ;
    skos:definition "Relates an expression to a work that contains a critical evaluation of a described expression."@en .

<http://rdaregistry.info/Elements/e/P20273> a rdf:Property ;
    rdfs:label "is evaluated in (expression)"@en ;
    rdakit:instructionNumber "23.5" ;
    rdakit:toolkitDefinition "A work that examines or judges a described expression."@en,
        "Una obra que examina o juzga la expresión descrita."@es,
        "Expression d’une œuvre qui examine ou juge l’expression décrite."@fr ;
    rdakit:toolkitLabel "evaluated in (expression)"@en,
        "evaluada en (expresión)"@es,
        "évalué dans (expression)"@fr ;
    reg:hasSubproperty <http://rdaregistry.info/Elements/e/object/P20273> ;
    reg:hasUnconstrained <http://rdaregistry.info/Elements/u/P60218> ;
    reg:lexicalAlias <http://rdaregistry.info/Elements/e/evaluatedInExpression.en> ;
    reg:name "evaluatedInExpression"@en ;
    reg:status <http://metadataregistry.org/uri/RegStatus/1001> ;
    rdfs:domain <http://rdaregistry.info/Elements/c/C10006> ;
    rdfs:isDefinedBy <http://rdaregistry.info/Elements/e/> ;
    rdfs:subPropertyOf <http://rdaregistry.info/Elements/e/P20269> ;
    skos:definition "Relates an expression to a work that examines or judges a described expression."@en .

<http://rdaregistry.info/Elements/e/P20274> a rdf:Property ;
    rdfs:label "is reviewed in (expression)"@en ;
    rdakit:instructionNumber "23.5" ;
    rdakit:toolkitDefinition "A work that contains a brief evaluation of a described expression."@en,
        "Una obra que contiene una evaluación breve de la expresión descrita."@es,
        "Expression d’une œuvre qui contient une brève évaluation de l’expression décrite."@fr ;
    rdakit:toolkitLabel "reviewed in (expression)"@en,
        "reseñada en (expresión)"@es,
        "recensé dans (expression)"@fr ;
    reg:hasSubproperty <http://rdaregistry.info/Elements/e/object/P20274> ;
    reg:hasUnconstrained <http://rdaregistry.info/Elements/u/P60211> ;
    reg:lexicalAlias <http://rdaregistry.info/Elements/e/reviewedInExpression.en> ;
    reg:name "reviewedInExpression"@en ;
    reg:status <http://metadataregistry.org/uri/RegStatus/1001> ;
    rdfs:domain <http://rdaregistry.info/Elements/c/C10006> ;
    rdfs:isDefinedBy <http://rdaregistry.info/Elements/e/> ;
    rdfs:subPropertyOf <http://rdaregistry.info/Elements/e/P20269> ;
    skos:definition "Relates an expression to a work that contains a brief evaluation of a described expression."@en .

<http://rdaregistry.info/Elements/e/P20275> a rdf:Property ;
    rdfs:label "has writer of foreword"@en ;
    rdakit:instructionNumber "18.5" ;
    rdakit:toolkitDefinition "An agent contributing to an expression of a work by providing a foreword to an original work."@en,
        "Una persona, familia o entidad corporativa que contribuye a una expresión de una obra proporcionando un prólogo a la obra original."@es ;
    rdakit:toolkitLabel "writer of foreword"@en,
        "escritor de prólogo"@es ;
    reg:hasSubproperty <http://rdaregistry.info/Elements/e/object/P20275> ;
    reg:hasUnconstrained <http://rdaregistry.info/Elements/u/P60809> ;
    reg:lexicalAlias <http://rdaregistry.info/Elements/e/writerOfForeword.en> ;
    reg:name "writerOfForeword"@en ;
    reg:status <http://metadataregistry.org/uri/RegStatus/1001> ;
    rdfs:domain <http://rdaregistry.info/Elements/c/C10006> ;
    rdfs:isDefinedBy <http://rdaregistry.info/Elements/e/> ;
    rdfs:subPropertyOf <http://rdaregistry.info/Elements/e/P20046> ;
    skos:definition "Relates an expression to an agent contributing to an expression of a work by providing a foreword to an original work."@en .

<http://rdaregistry.info/Elements/e/P20276> a rdf:Property ;
    rdfs:label "has sound designer"@en ;
    rdakit:instructionNumber "18.5" ;
    rdakit:toolkitDefinition "An agent contributing to an expression of a work by designing and creating audio/sound components."@en,
        "Una persona, familia o entidad corporativa que contribuye a una expresión de una obra mediante el diseño y la creación de componentes de sonido."@es ;
    rdakit:toolkitLabel "sound designer"@en,
        "diseñador de sonido"@es ;
    reg:hasSubproperty <http://rdaregistry.info/Elements/e/object/P20276> ;
    reg:hasUnconstrained <http://rdaregistry.info/Elements/u/P60811> ;
    reg:lexicalAlias <http://rdaregistry.info/Elements/e/soundDesigner.en> ;
    reg:name "soundDesigner"@en ;
    reg:status <http://metadataregistry.org/uri/RegStatus/1001> ;
    rdfs:domain <http://rdaregistry.info/Elements/c/C10006> ;
    rdfs:isDefinedBy <http://rdaregistry.info/Elements/e/> ;
    rdfs:subPropertyOf <http://rdaregistry.info/Elements/e/P20053> ;
    skos:definition "Relates an expression to an agent contributing to an expression of a work by designing and creating audio/sound components."@en .

<http://rdaregistry.info/Elements/e/P20277> a rdf:Property ;
    rdfs:label "has lighting designer"@en ;
    rdakit:instructionNumber "18.5" ;
    rdakit:toolkitDefinition "An agent contributing to an expression of a work by designing and creating lighting components."@en,
        "Una persona, familia o entidad corporativa que contribuye a una expresión de una obra mediante el diseño y la creación de componentes de iluminación."@es ;
    rdakit:toolkitLabel "lighting designer"@en,
        "diseñador de iluminación"@es ;
    reg:hasSubproperty <http://rdaregistry.info/Elements/e/object/P20277> ;
    reg:hasUnconstrained <http://rdaregistry.info/Elements/u/P60813> ;
    reg:lexicalAlias <http://rdaregistry.info/Elements/e/lightingDesigner.en> ;
    reg:name "lightingDesigner"@en ;
    reg:status <http://metadataregistry.org/uri/RegStatus/1001> ;
    rdfs:domain <http://rdaregistry.info/Elements/c/C10006> ;
    rdfs:isDefinedBy <http://rdaregistry.info/Elements/e/> ;
    rdfs:subPropertyOf <http://rdaregistry.info/Elements/e/P20053> ;
    skos:definition "Relates an expression to an agent contributing to an expression of a work by designing and creating lighting components."@en .

<http://rdaregistry.info/Elements/e/P20280> a rdf:Property ;
    rdfs:label "has software developer"@en ;
    rdakit:instructionNumber "18.5" ;
    rdakit:toolkitDefinition "An agent contributing to an expression of a work by researching, designing, implementing, or testing software."@en,
        "Una persona, familia o entidad corporativa que contribuye a una expresión de una obra mediante la investigación, diseño, implementación, y la realización de pruebas del software."@es ;
    rdakit:toolkitLabel "software developer"@en,
        "desarrollador de software"@es ;
    reg:hasSubproperty <http://rdaregistry.info/Elements/e/object/P20280> ;
    reg:hasUnconstrained <http://rdaregistry.info/Elements/u/P60828> ;
    reg:lexicalAlias <http://rdaregistry.info/Elements/e/softwareDeveloper.en> ;
    reg:name "softwareDeveloper"@en ;
    reg:status <http://metadataregistry.org/uri/RegStatus/1001> ;
    rdfs:domain <http://rdaregistry.info/Elements/c/C10006> ;
    rdfs:isDefinedBy <http://rdaregistry.info/Elements/e/> ;
    rdfs:subPropertyOf <http://rdaregistry.info/Elements/e/P20053> ;
    skos:definition "Relates an expression to an agent contributing to an expression of a work by researching, designing, implementing, or testing software."@en .

<http://rdaregistry.info/Elements/e/P20281> a rdf:Property ;
    rdfs:label "is oratorio adaptation of (expression)"@en ;
    rdakit:instructionNumber "24.5" ;
    rdakit:toolkitDefinition "An expression of a work that has been adapted as an oratorio."@en,
        "Una expresión de una obra que ha sido adaptada como un oratorio."@es ;
    rdakit:toolkitLabel "oratorio adaptation of (expression)"@en,
        "adaptación para oratorio de (expresión)"@es ;
    reg:hasSubproperty <http://rdaregistry.info/Elements/e/object/P20281> ;
    reg:hasUnconstrained <http://rdaregistry.info/Elements/u/P60830> ;
    reg:lexicalAlias <http://rdaregistry.info/Elements/e/oratorioAdaptationOfExpression.en> ;
    reg:name "oratorioAdaptationOfExpression"@en ;
    reg:status <http://metadataregistry.org/uri/RegStatus/1001> ;
    rdfs:domain <http://rdaregistry.info/Elements/c/C10006> ;
    rdfs:isDefinedBy <http://rdaregistry.info/Elements/e/> ;
    rdfs:subPropertyOf <http://rdaregistry.info/Elements/e/P20152> ;
    skos:definition "Relates an expression to an expression of a work that has been adapted as an oratorio."@en .

<http://rdaregistry.info/Elements/e/P20282> a rdf:Property ;
    rdfs:label "is adapted as oratorio (expression)"@en ;
    rdakit:instructionNumber "24.5" ;
    rdakit:toolkitDefinition "An expression of an oratorio based on a source expression."@en,
        "Una expresión de un oratorio basada en la expresión fuente."@es ;
    rdakit:toolkitLabel "adapted as oratorio (expression)"@en,
        "adaptada como oratorio (expresión)"@es ;
    reg:hasSubproperty <http://rdaregistry.info/Elements/e/object/P20282> ;
    reg:hasUnconstrained <http://rdaregistry.info/Elements/u/P60831> ;
    reg:lexicalAlias <http://rdaregistry.info/Elements/e/adaptedAsOratorioExpression.en> ;
    reg:name "adaptedAsOratorioExpression"@en ;
    reg:status <http://metadataregistry.org/uri/RegStatus/1001> ;
    rdfs:domain <http://rdaregistry.info/Elements/c/C10006> ;
    rdfs:isDefinedBy <http://rdaregistry.info/Elements/e/> ;
    rdfs:subPropertyOf <http://rdaregistry.info/Elements/e/P20153> ;
    skos:definition "Relates an expression to an expression of an oratorio based on a source expression."@en .

<http://rdaregistry.info/Elements/e/P20283> a rdf:Property ;
    rdfs:label "has colourist"@en ;
    rdakit:instructionNumber "18.5" ;
    rdakit:toolkitDefinition "An agent contributing to an expression of a work by applying colour to drawings, prints, photographs, maps, moving images, etc."@en,
        "Una persona, familia o entidad corporativa que contribuye a una expresión de una obra aplicando color a los dibujos, grabados, fotografías, mapas, imágenes en movimiento, etc."@es ;
    rdakit:toolkitLabel "colourist"@en,
        "colorista"@es ;
    reg:hasSubproperty <http://rdaregistry.info/Elements/e/object/P20283> ;
    reg:hasUnconstrained <http://rdaregistry.info/Elements/u/P60838> ;
    reg:lexicalAlias <http://rdaregistry.info/Elements/e/colourist.en> ;
    reg:name "colourist"@en ;
    reg:status <http://metadataregistry.org/uri/RegStatus/1001> ;
    rdfs:domain <http://rdaregistry.info/Elements/c/C10006> ;
    rdfs:isDefinedBy <http://rdaregistry.info/Elements/e/> ;
    rdfs:subPropertyOf <http://rdaregistry.info/Elements/e/P20053> ;
    skos:definition "Relates an expression to an agent contributing to an expression of a work by applying colour to drawings, prints, photographs, maps, moving images, etc."@en .

<http://rdaregistry.info/Elements/e/P20284> a rdf:Property ;
    rdfs:label "has make-up artist"@en ;
    rdakit:instructionNumber "18.5" ;
    rdakit:toolkitDefinition "An agent contributing to an expression of a work by applying make-up and prosthetics for a moving image production or for a musical or dramatic presentation or entertainment."@en,
        "Una persona, familia o entidad corporativa que contribuye a una expresión de una obra mediante la aplicación de maquillaje y prótesis para una producción de imágenes en movimiento o para una presentación o espectáculo musical o dramático."@es ;
    rdakit:toolkitLabel "make-up artist"@en,
        "maquillador"@es ;
    reg:hasSubproperty <http://rdaregistry.info/Elements/e/object/P20284> ;
    reg:hasUnconstrained <http://rdaregistry.info/Elements/u/P60840> ;
    reg:lexicalAlias <http://rdaregistry.info/Elements/e/makeUpArtist.en> ;
    reg:name "makeUpArtist"@en ;
    reg:status <http://metadataregistry.org/uri/RegStatus/1001> ;
    rdfs:domain <http://rdaregistry.info/Elements/c/C10006> ;
    rdfs:isDefinedBy <http://rdaregistry.info/Elements/e/> ;
    rdfs:subPropertyOf <http://rdaregistry.info/Elements/e/P20053> ;
    skos:definition "Relates an expression to an agent contributing to an expression of a work by applying make-up and prosthetics for a moving image production or for a musical or dramatic presentation or entertainment."@en .

<http://rdaregistry.info/Elements/e/P20285> a rdf:Property ;
    rdfs:label "has choral conductor"@en ;
    rdakit:instructionNumber "18.5" ;
    rdakit:toolkitDefinition "A conductor contributing to an expression of a musical work by leading a choral performing group in a musical or dramatic presentation, etc."@en,
        "Un intérprete que contribuye a la expresión de una obra musical dirigiendo un grupo de interpretación coral en una presentación musical o teatral, etc."@es ;
    rdakit:toolkitLabel "choral conductor"@en,
        "director de coro"@es ;
    reg:hasSubproperty <http://rdaregistry.info/Elements/e/object/P20285> ;
    reg:hasUnconstrained <http://rdaregistry.info/Elements/u/P60842> ;
    reg:lexicalAlias <http://rdaregistry.info/Elements/e/choralConductor.en> ;
    reg:name "choralConductor"@en ;
    reg:status <http://metadataregistry.org/uri/RegStatus/1001> ;
    rdfs:domain <http://rdaregistry.info/Elements/c/C10006> ;
    rdfs:isDefinedBy <http://rdaregistry.info/Elements/e/> ;
    rdfs:subPropertyOf <http://rdaregistry.info/Elements/e/P20011> ;
    skos:definition "Relates an expression to a conductor contributing to an expression of a musical work by leading a choral performing group in a musical or dramatic presentation, etc."@en .

<http://rdaregistry.info/Elements/e/P20286> a rdf:Property ;
    rdfs:label "has instrumental conductor"@en ;
    rdakit:instructionNumber "18.5" ;
    rdakit:toolkitDefinition "A conductor contributing to an expression of a musical work by leading an instrumental performing group in a musical or dramatic presentation, etc."@en,
        "Un intérprete que contribuye a la expresión de una obra musical dirigiendo un grupo de interpretación instrumental en una presentación musical o teatral, etc."@es ;
    rdakit:toolkitLabel "instrumental conductor"@en,
        "director instrumental"@es ;
    reg:hasSubproperty <http://rdaregistry.info/Elements/e/object/P20286> ;
    reg:hasUnconstrained <http://rdaregistry.info/Elements/u/P60844> ;
    reg:lexicalAlias <http://rdaregistry.info/Elements/e/instrumentalConductor.en> ;
    reg:name "instrumentalConductor"@en ;
    reg:status <http://metadataregistry.org/uri/RegStatus/1001> ;
    rdfs:domain <http://rdaregistry.info/Elements/c/C10006> ;
    rdfs:isDefinedBy <http://rdaregistry.info/Elements/e/> ;
    rdfs:subPropertyOf <http://rdaregistry.info/Elements/e/P20011> ;
    skos:definition "Relates an expression to a conductor contributing to an expression of a musical work by leading an instrumental performing group in a musical or dramatic presentation, etc."@en .

<http://rdaregistry.info/Elements/e/P20287> a rdf:Property ;
    rdfs:label "has censor"@en ;
    rdakit:instructionNumber "18.5" ;
    rdakit:seeAlso <http://rdaregistry.info/Elements/w/P10061> ;
    rdakit:toolkitDefinition "An agent contributing to an expression of a work by revising the content for the purpose of suppressing parts deemed objectionable on moral, political, military, or other grounds, but leaving the nature and content substantially unchanged."@en ;
    rdakit:toolkitLabel "censor"@en ;
    reg:hasSubproperty <http://rdaregistry.info/Elements/e/object/P20287> ;
    reg:hasUnconstrained <http://rdaregistry.info/Elements/u/P60851> ;
    reg:lexicalAlias <http://rdaregistry.info/Elements/e/censor.en> ;
    reg:name "censor"@en ;
    reg:status <http://metadataregistry.org/uri/RegStatus/1001> ;
    rdfs:domain <http://rdaregistry.info/Elements/c/C10006> ;
    rdfs:isDefinedBy <http://rdaregistry.info/Elements/e/> ;
    rdfs:subPropertyOf <http://rdaregistry.info/Elements/e/P20053> ;
    skos:definition "Relates an expression to an agent contributing to an expression of a work by revising the content for the purpose of suppressing parts deemed objectionable on moral, political, military, or other grounds, but leaving the nature and content substantially unchanged."@en ;
    skos:scopeNote "Substantial modification that results in the creation of a new work is excluded."@en .

<http://rdaregistry.info/Elements/e/P20288> a rdf:Property ;
    rdfs:label "has photographer (expression)"@en ;
    rdakit:instructionNumber "18.5" ;
    rdakit:seeAlso <http://rdaregistry.info/Elements/w/P10056> ;
    rdakit:toolkitDefinition "An illustrator contributing to an expression of a work by providing supplementary photographic content to an original work."@en ;
    rdakit:toolkitLabel "photographer (expression)"@en ;
    reg:hasSubproperty <http://rdaregistry.info/Elements/e/object/P20288> ;
    reg:hasUnconstrained <http://rdaregistry.info/Elements/u/P60429> ;
    reg:lexicalAlias <http://rdaregistry.info/Elements/e/photographerExpression.en> ;
    reg:name "photographerExpression"@en ;
    reg:status <http://metadataregistry.org/uri/RegStatus/1001> ;
    rdfs:domain <http://rdaregistry.info/Elements/c/C10006> ;
    rdfs:isDefinedBy <http://rdaregistry.info/Elements/e/> ;
    rdfs:subPropertyOf <http://rdaregistry.info/Elements/e/P20051> ;
    skos:definition "Relates an expression to an illustrator contributing to an expression of a work by providing supplementary photographic content to an original work."@en ;
    skos:scopeNote "Creation of content that is primarily artistic is excluded."@en .

<http://rdaregistry.info/Elements/e/P20289> a rdf:Property ;
    rdfs:label "has restorationist (expression)"@en ;
    rdakit:instructionNumber "18.5" ;
    rdakit:toolkitDefinition "An agent who contributes to an expression of a work by restoring and/or combining earlier expressions, which may be damaged or fragmentary, to create a new expression."@en ;
    rdakit:toolkitLabel "restorationist (expression)"@en ;
    reg:hasSubproperty <http://rdaregistry.info/Elements/e/object/P20289> ;
    reg:hasUnconstrained <http://rdaregistry.info/Elements/u/P60450> ;
    reg:lexicalAlias <http://rdaregistry.info/Elements/e/restorationistExpression.en> ;
    reg:name "restorationistExpression"@en ;
    reg:status <http://metadataregistry.org/uri/RegStatus/1001> ;
    rdfs:domain <http://rdaregistry.info/Elements/c/C10006> ;
    rdfs:isDefinedBy <http://rdaregistry.info/Elements/e/> ;
    rdfs:subPropertyOf <http://rdaregistry.info/Elements/e/P20053> ;
    skos:definition "Relates an expression to an agent who contributes to an expression of a work by restoring and/or combining earlier expressions, which may be damaged or fragmentary, to create a new expression."@en .

<http://rdaregistry.info/Elements/e/P20294> a rdf:Property ;
    rdfs:label "has music programmer"@en ;
    rdakit:instructionNumber "18.5" ;
    rdakit:seeAlso <http://rdaregistry.info/Elements/w/P10053> ;
    rdakit:toolkitDefinition "An agent contributing to an expression of a musical work by using electronic audio devices and/or computer software to generate sounds."@en ;
    rdakit:toolkitLabel "music programmer"@en ;
    reg:hasSubproperty <http://rdaregistry.info/Elements/e/object/P20294> ;
    reg:hasUnconstrained <http://rdaregistry.info/Elements/u/P60894> ;
    reg:lexicalAlias <http://rdaregistry.info/Elements/e/musicProgrammer.en> ;
    reg:name "musicProgrammer"@en ;
    reg:status <http://metadataregistry.org/uri/RegStatus/1001> ;
    rdfs:domain <http://rdaregistry.info/Elements/c/C10006> ;
    rdfs:isDefinedBy <http://rdaregistry.info/Elements/e/> ;
    rdfs:subPropertyOf <http://rdaregistry.info/Elements/e/P20053> ;
    skos:definition "Relates an expression to an agent contributing to an expression of a musical work by using electronic audio devices and/or computer software to generate sounds."@en,
        "Relates an expression to an agent contributing to an expression of a musical work by using electronic audio devices or computer software to generate sounds."@en ;
    skos:scopeNote "The creation of a new musical work is excluded."@en .

<http://rdaregistry.info/Elements/e/P20295> a rdf:Property ;
    rdfs:label "has dubbing director"@en ;
    rdakit:instructionNumber "18.5" ;
    rdakit:toolkitDefinition "An agent responsible for the general management and supervision of the process of adding new dialogue or other sounds to complete a sound track for an expression."@en ;
    rdakit:toolkitLabel "dubbing director"@en ;
    reg:hasSubproperty <http://rdaregistry.info/Elements/e/object/P20295> ;
    reg:hasUnconstrained <http://rdaregistry.info/Elements/u/P60895> ;
    reg:lexicalAlias <http://rdaregistry.info/Elements/e/dubbingDirector.en> ;
    reg:name "dubbingDirector"@en ;
    reg:status <http://metadataregistry.org/uri/RegStatus/1001> ;
    rdfs:domain <http://rdaregistry.info/Elements/c/C10006> ;
    rdfs:isDefinedBy <http://rdaregistry.info/Elements/e/> ;
    rdfs:subPropertyOf <http://rdaregistry.info/Elements/e/P20053> ;
    skos:definition "Relates an expression to an agent responsible for the general management and supervision of the process of adding new dialogue or other sounds to complete a sound track for an expression."@en .

<http://rdaregistry.info/Elements/e/P20296> a rdf:Property ;
    rdfs:label "has DJ"@en ;
    rdakit:instructionNumber "18.5" ;
    rdakit:seeAlso <http://rdaregistry.info/Elements/e/P20293> ;
    rdakit:toolkitDefinition "An agent who mixes recorded tracks together during a live performance or in a recording studio to appear as one continuous track."@en ;
    rdakit:toolkitLabel "DJ"@en ;
    reg:hasSubproperty <http://rdaregistry.info/Elements/e/object/P20296> ;
    reg:hasUnconstrained <http://rdaregistry.info/Elements/u/P60896> ;
    reg:lexicalAlias <http://rdaregistry.info/Elements/e/DJ.en> ;
    reg:name "DJ"@en ;
    reg:status <http://metadataregistry.org/uri/RegStatus/1001> ;
    rdfs:domain <http://rdaregistry.info/Elements/c/C10006> ;
    rdfs:isDefinedBy <http://rdaregistry.info/Elements/e/> ;
    rdfs:subPropertyOf <http://rdaregistry.info/Elements/e/P20053> ;
    skos:definition "Relates an expression to an agent who mixes recorded tracks together during a live performance or in a recording studio to appear as one continuous track."@en ;
    skos:scopeNote "Remixing activities that substantially change the nature and content of an original work, resulting in a new work, and mixing and assembling the multiple tracks of a recording are excluded."@en .

<http://rdaregistry.info/Elements/e/P20012> a rdf:Property ;
    rdfs:label "has actor"@en ;
    rdakit:instructionNumber "18.5" ;
    rdakit:toolkitDefinition "A performer contributing to an expression of a work by acting as a cast member or player in a musical or dramatic presentation, etc."@en,
        "Un intérprete que contribuye a una expresión de una obra actuando como un miembro de un reparto o actor en una producción musical o teatral, etc."@es,
        "Interprète contribuant à une expression d’une œuvre en agissant à titre de membre d’une distribution artistique ou de comédien dans une représentation musicale ou dramatique, etc."@fr ;
    rdakit:toolkitLabel "actor"@en,
        "actor"@es,
        "acteur"@fr ;
    reg:hasSubproperty <http://rdaregistry.info/Elements/e/P20070>,
        <http://rdaregistry.info/Elements/e/object/P20012> ;
    reg:hasUnconstrained <http://rdaregistry.info/Elements/u/P60142> ;
    reg:lexicalAlias <http://rdaregistry.info/Elements/e/actor.en> ;
    reg:name "actor"@en ;
    reg:status <http://metadataregistry.org/uri/RegStatus/1001> ;
    rdfs:domain <http://rdaregistry.info/Elements/c/C10006> ;
    rdfs:isDefinedBy <http://rdaregistry.info/Elements/e/> ;
    rdfs:subPropertyOf <http://rdaregistry.info/Elements/e/P20039> ;
    skos:definition "Relates an expression to a performer contributing to an expression of a work by acting as a cast member or player in a musical or dramatic presentation, etc."@en .

<http://rdaregistry.info/Elements/e/P20013> a rdf:Property ;
    rdfs:label "has on-screen presenter"@en ;
    rdakit:instructionNumber "18.5" ;
    rdakit:seeAlso <http://rdaregistry.info/Elements/e/P20279> ;
    rdakit:toolkitDefinition "A performer contributing to an expression of a work by appearing on screen to provide contextual or background information."@en,
        "Un intérprete que contribuye a una expresión de una obra para ofrecer en pantalla información contextual o básica."@es,
        "Interprète contribuant à une expression d’une œuvre en apparaissant à l’écran pour fournir de l’information contextuelle ou complémentaire."@fr ;
    rdakit:toolkitLabel "on-screen presenter"@en,
        "presentador en pantalla"@es,
        "présentateur à l’écran"@fr ;
    reg:hasSubproperty <http://rdaregistry.info/Elements/e/object/P20013> ;
    reg:hasUnconstrained <http://rdaregistry.info/Elements/u/P60143> ;
    reg:lexicalAlias <http://rdaregistry.info/Elements/e/onScreenPresenter.en> ;
    reg:name "onScreenPresenter"@en ;
    reg:status <http://metadataregistry.org/uri/RegStatus/1001> ;
    rdfs:domain <http://rdaregistry.info/Elements/c/C10006> ;
    rdfs:isDefinedBy <http://rdaregistry.info/Elements/e/> ;
    rdfs:subPropertyOf <http://rdaregistry.info/Elements/e/P20039> ;
    skos:definition "Relates an expression to a performer contributing to an expression of a work by appearing on screen to provide contextual or background information."@en ;
    skos:scopeNote "Appearance in nonfiction moving image materials or in introductions to fiction moving image materials is included. Appearance on screen in a non-performing role is excluded."@en .

<http://rdaregistry.info/Elements/e/P20029> a rdf:Property ;
    rdfs:label "has arranger of music"@en ;
    rdakit:instructionNumber "18.5" ;
    rdakit:seeAlso <http://rdaregistry.info/Elements/w/P10053> ;
    rdakit:toolkitDefinition "An agent contributing to an expression of a musical work by rewriting a composition for a medium of performance different from that for which a work was originally intended."@en,
        "Una persona, familia o entidad corporativa que contribuye a una expresión de una obra musical reescribiendo la composición para un medio de una interpretación diferente de aquel para el que se habia concebido la obra."@es,
        "Personne, famille ou collectivité contribuant à une expression d’une œuvre musicale en réécrivant la composition pour une distribution d’exécution différente de celle à laquelle l’œuvre est originellement destinée."@fr ;
    rdakit:toolkitLabel "arranger of music"@en,
        "arreglista musical"@es,
        "arrangeur de musique"@fr ;
    reg:hasSubproperty <http://rdaregistry.info/Elements/e/object/P20029> ;
    reg:hasUnconstrained <http://rdaregistry.info/Elements/u/P60379> ;
    reg:lexicalAlias <http://rdaregistry.info/Elements/e/arrangerOfMusic.en> ;
    reg:name "arrangerOfMusic"@en ;
    reg:status <http://metadataregistry.org/uri/RegStatus/1001> ;
    rdfs:domain <http://rdaregistry.info/Elements/c/C10006> ;
    rdfs:isDefinedBy <http://rdaregistry.info/Elements/e/> ;
    rdfs:subPropertyOf <http://rdaregistry.info/Elements/e/P20053> ;
    skos:definition "Relates an expression to an agent contributing to an expression of a musical work by rewriting a composition for a medium of performance different from that for which a work was originally intended."@en ;
    skos:scopeNote "Contribution includes modification of a work for the same medium of performance, etc., keeping the musical substance of the original composition essentially unchanged, and excludes substantial modification that results in the creation of a new musical work."@en .

<http://rdaregistry.info/Elements/e/P20030> a rdf:Property ;
    rdfs:label "has writer of added text"@en ;
    rdakit:instructionNumber "18.5" ;
    rdakit:toolkitDefinition "An agent contributing to an expression of a primarily non-textual work by providing text, such as writing captions for photographs or descriptions of maps."@en,
        "Una persona, familia o entidad corporativa que contribuye a una expresión de una obra que no es básicamente texto ofreciendo texto para la obra no textual (por ej., titulación de fotografías, descripción de mapas)."@es,
        "Personne, famille ou collectivité contribuant à une expression d’une œuvre essentiellement non textuelle en fournissant un texte pour l’œuvre non textuelle (par exemple, en écrivant des légendes pour des photographies, des descriptions de cartes géographiques)."@fr ;
    rdakit:toolkitLabel "writer of added text"@en,
        "autor de texto adicional"@es,
        "auteur de texte ajouté"@fr ;
    reg:hasSubproperty <http://rdaregistry.info/Elements/e/P20068>,
        <http://rdaregistry.info/Elements/e/object/P20030> ;
    reg:hasUnconstrained <http://rdaregistry.info/Elements/u/P60380> ;
    reg:lexicalAlias <http://rdaregistry.info/Elements/e/writerOfAddedText.en> ;
    reg:name "writerOfAddedText"@en ;
    reg:status <http://metadataregistry.org/uri/RegStatus/1001> ;
    rdfs:domain <http://rdaregistry.info/Elements/c/C10006> ;
    rdfs:isDefinedBy <http://rdaregistry.info/Elements/e/> ;
    rdfs:subPropertyOf <http://rdaregistry.info/Elements/e/P20046> ;
    skos:definition "Relates an expression to an agent contributing to an expression of a primarily non-textual work by providing text, such as writing captions for photographs or descriptions of maps."@en .

<http://rdaregistry.info/Elements/e/P20071> a rdf:Property ;
    rdfs:label "has note on expression"@en ;
    rdakit:instructionNumber "7.29" ;
    rdakit:toolkitDefinition "A note providing additional information about content recorded as an expression attribute."@en,
        "Una anotación que proporciona información adicional sobre contenido registrado como un atributo de la expresión."@es,
        "Annotation fournissant un complément d’information relatif au contenu enregistré comme attribut de l’expression."@fr ;
    rdakit:toolkitLabel "note on expression"@en,
        "nota sobre la expresión"@es,
        "note relative à l’expression"@fr ;
    reg:hasSubproperty <http://rdaregistry.info/Elements/e/P20010> ;
    reg:hasUnconstrained <http://rdaregistry.info/Elements/u/P60470> ;
    reg:lexicalAlias <http://rdaregistry.info/Elements/e/noteOnExpression.en> ;
    reg:name "noteOnExpression"@en ;
    reg:status <http://metadataregistry.org/uri/RegStatus/1001> ;
    rdfs:domain <http://rdaregistry.info/Elements/c/C10006> ;
    rdfs:isDefinedBy <http://rdaregistry.info/Elements/e/> ;
    skos:definition "Relates an expression to a note providing additional information about content recorded as an expression attribute."@en .

<http://rdaregistry.info/Elements/e/P20114> a rdf:Property ;
    rdfs:label "is imitated as (expression)"@en ;
    rdakit:instructionNumber "24.5" ;
    rdakit:toolkitDefinition "An expression of a work that copies the style or content of the source work."@en,
        "Una expresión de una obra que copia el estilo o contenido de la obra fuente."@es,
        "Expression d’une œuvre qui copie le style ou le contenu de l’œuvre source."@fr ;
    rdakit:toolkitLabel "imitated as (expression)"@en,
        "imitada como (expresión)"@es,
        "imité comme (expression)"@fr ;
    reg:hasSubproperty <http://rdaregistry.info/Elements/e/P20142>,
        <http://rdaregistry.info/Elements/e/object/P20114> ;
    reg:hasUnconstrained <http://rdaregistry.info/Elements/u/P60214> ;
    reg:lexicalAlias <http://rdaregistry.info/Elements/e/imitatedAsExpression.en> ;
    reg:name "imitatedAsExpression"@en ;
    reg:status <http://metadataregistry.org/uri/RegStatus/1001> ;
    rdfs:domain <http://rdaregistry.info/Elements/c/C10006> ;
    rdfs:isDefinedBy <http://rdaregistry.info/Elements/e/> ;
    rdfs:subPropertyOf <http://rdaregistry.info/Elements/e/P20203> ;
    skos:definition "Relates an expression to an expression of a work that copies the style or content of a source work."@en .

<http://rdaregistry.info/Elements/e/P20141> a rdf:Property ;
    rdfs:label "is translation of"@en ;
    rdakit:instructionNumber "24.5" ;
    rdakit:toolkitDefinition "An expression of a work that has been translated, i.e., the text expressed in a language different from that of an original work."@en,
        "Una expresión de una obra que fue traducida, i.e., el texto expresado en una lengua diferente de la utilizada en la obra original."@es,
        "Expression d’une œuvre qui a été traduite, c’est-à-dire dont le texte a été exprimé dans une langue différente de celle de l’œuvre d’origine."@fr ;
    rdakit:toolkitLabel "translation of"@en,
        "traducción de"@es,
        "traduction de"@fr ;
    reg:hasSubproperty <http://rdaregistry.info/Elements/e/P20078>,
        <http://rdaregistry.info/Elements/e/object/P20141> ;
    reg:hasUnconstrained <http://rdaregistry.info/Elements/u/P60244> ;
    reg:lexicalAlias <http://rdaregistry.info/Elements/e/translationOf.en> ;
    reg:name "translationOf"@en ;
    reg:status <http://metadataregistry.org/uri/RegStatus/1001> ;
    rdfs:domain <http://rdaregistry.info/Elements/c/C10006> ;
    rdfs:isDefinedBy <http://rdaregistry.info/Elements/e/> ;
    rdfs:subPropertyOf <http://rdaregistry.info/Elements/e/P20204> ;
    skos:definition "Relates an expression to an expression of a work that has been translated, i.e., the text expressed in a language different from that of an original work."@en .

<http://rdaregistry.info/Elements/e/P20171> a rdf:Property ;
    rdfs:label "is translated as"@en ;
    rdakit:instructionNumber "24.5" ;
    rdakit:toolkitDefinition "An expression of a work that translates the text of a source expression into a language different from that of an original work."@en,
        "Una expresión de una obra que traduce el texto de una expresión fuente a una lengua diferente a la de la obra original."@es,
        "Expression d’une œuvre qui traduit le texte de l’expression source dans une langue différente de celle de l’œuvre d’origine."@fr ;
    rdakit:toolkitLabel "translated as"@en,
        "traducida como"@es,
        "traduit comme"@fr ;
    reg:hasSubproperty <http://rdaregistry.info/Elements/e/P20079>,
        <http://rdaregistry.info/Elements/e/object/P20171> ;
    reg:hasUnconstrained <http://rdaregistry.info/Elements/u/P60280> ;
    reg:lexicalAlias <http://rdaregistry.info/Elements/e/translatedAs.en> ;
    reg:name "translatedAs"@en ;
    reg:status <http://metadataregistry.org/uri/RegStatus/1001> ;
    rdfs:domain <http://rdaregistry.info/Elements/c/C10006> ;
    rdfs:isDefinedBy <http://rdaregistry.info/Elements/e/> ;
    rdfs:subPropertyOf <http://rdaregistry.info/Elements/e/P20203> ;
    skos:definition "Relates an expression to an expression of a work that translates the text of a source expression into a language different from that of an original work."@en .

<http://rdaregistry.info/Elements/e/P20195> a rdf:Property ;
    rdfs:label "is imitation of (expression)"@en ;
    rdakit:instructionNumber "24.5" ;
    rdakit:toolkitDefinition "An expression of a work whose style or content is copied in a derivative work."@en,
        "Una expresión de una obra cuyo estilo o contenido es copiado en una obra derivada."@es,
        "Expression d’une œuvre dont le style ou le contenu est copié dans une œuvre dérivée."@fr ;
    rdakit:toolkitLabel "imitation of (expression)"@en,
        "imitación de (expresión)"@es,
        "imitation de (expression)"@fr ;
    reg:hasSubproperty <http://rdaregistry.info/Elements/e/P20196>,
        <http://rdaregistry.info/Elements/e/object/P20195> ;
    reg:hasUnconstrained <http://rdaregistry.info/Elements/u/P60311> ;
    reg:lexicalAlias <http://rdaregistry.info/Elements/e/imitationOfExpression.en> ;
    reg:name "imitationOfExpression"@en ;
    reg:status <http://metadataregistry.org/uri/RegStatus/1001> ;
    rdfs:domain <http://rdaregistry.info/Elements/c/C10006> ;
    rdfs:isDefinedBy <http://rdaregistry.info/Elements/e/> ;
    rdfs:subPropertyOf <http://rdaregistry.info/Elements/e/P20204> ;
    skos:definition "Relates an expression to an expression of a work whose style or content is copied in a derivative work."@en .

<http://rdaregistry.info/Elements/e/P20205> a rdf:Property ;
    rdfs:label "has related expression (expression)"@en,
        "har relaterat uttryck"@sv ;
    rdakit:toolkitLabel "relaterat uttryck"@sv ;
    reg:hasSubproperty <http://rdaregistry.info/Elements/e/P20232>,
        <http://rdaregistry.info/Elements/e/P20234>,
        <http://rdaregistry.info/Elements/e/datatype/P20205>,
        <http://rdaregistry.info/Elements/e/object/P20205> ;
    reg:hasUnconstrained <http://rdaregistry.info/Elements/u/P60313> ;
    reg:lexicalAlias <http://rdaregistry.info/Elements/e/relatedExpressionExpression.en> ;
    reg:name "relatedExpressionExpression"@en ;
    reg:status <http://metadataregistry.org/uri/RegStatus/1001> ;
    rdfs:domain <http://rdaregistry.info/Elements/c/C10006> ;
    rdfs:isDefinedBy <http://rdaregistry.info/Elements/e/> ;
    rdfs:subPropertyOf <http://rdaregistry.info/Elements/e/P20297> ;
    skos:definition "Relates an expression to an expression associated with an expression being described."@en .

<http://rdaregistry.info/Elements/e/P20233> a rdf:Property ;
    rdfs:label "has derivative expression relationship"@en ;
    rdakit:toolkitDefinition "An expression of a work that is based on or is a derivative of another expression."@en,
        "Una expresión de una obra que se basa en, o es una derivada de la expresión."@es,
        "Expression d’une œuvre qui est basée sur l’expression ou en constitue un dérivé."@fr ;
    rdakit:toolkitLabel "derivative expression relationship"@en,
        "relaciones de expresión derivada"@es,
        "relation d’expression dérivée"@fr ;
    reg:hasSubproperty <http://rdaregistry.info/Elements/e/P20203>,
        <http://rdaregistry.info/Elements/e/object/P20233> ;
    reg:lexicalAlias <http://rdaregistry.info/Elements/e/derivativeExpressionRelationship.en> ;
    reg:name "derivativeExpressionRelationship"@en ;
    reg:status <http://metadataregistry.org/uri/RegStatus/1001> ;
    rdfs:isDefinedBy <http://rdaregistry.info/Elements/e/> ;
    skos:definition "Relates an expression to an expression of a work that is based on or is a derivative of another expression."@en .

<http://rdaregistry.info/Elements/e/P20235> a rdf:Property ;
    rdfs:label "has sequential expression relationship"@en ;
    rdakit:toolkitDefinition "An expression of a work that is preceded by or succeeded by another expression."@en,
        "Una expresión de una obra que es precedida por o sucedida por la expresión."@es,
        "Expression d’une œuvre qui est précédée ou suivie par l’expression."@fr ;
    rdakit:toolkitLabel "sequential expression relationship"@en,
        "relaciones de expresión secuencial"@es,
        "relation d’expression séquentielle"@fr ;
    reg:hasSubproperty <http://rdaregistry.info/Elements/e/P20154>,
        <http://rdaregistry.info/Elements/e/P20169>,
        <http://rdaregistry.info/Elements/e/object/P20235> ;
    reg:lexicalAlias <http://rdaregistry.info/Elements/e/sequentialExpressionRelationship.en> ;
    reg:name "sequentialExpressionRelationship"@en ;
    reg:status <http://metadataregistry.org/uri/RegStatus/1001> ;
    rdfs:isDefinedBy <http://rdaregistry.info/Elements/e/> ;
    skos:definition "Relates an expression to an expression of a work that is preceded by or succeeded by another expression."@en .

<http://rdaregistry.info/Elements/e/P20236> a rdf:Property ;
    rdfs:label "has whole-part expression relationship"@en ;
    rdakit:toolkitDefinition "An expression that is contained in or contains another expression."@en,
        "Una expresión que es incluida en, o contiene la expresión."@es,
        "Expression d’une œuvre qui est contenue dans l’expression ou la contient."@fr ;
    rdakit:toolkitLabel "whole-part expression relationship"@en,
        "relación de la expresión todo-parte"@es,
        "relation d’expression tout-partie"@fr ;
    reg:hasSubproperty <http://rdaregistry.info/Elements/e/P20074>,
        <http://rdaregistry.info/Elements/e/P20145>,
        <http://rdaregistry.info/Elements/e/object/P20236> ;
    reg:lexicalAlias <http://rdaregistry.info/Elements/e/wholePartExpressionRelationship.en> ;
    reg:name "wholePartExpressionRelationship"@en ;
    reg:status <http://metadataregistry.org/uri/RegStatus/1001> ;
    rdfs:isDefinedBy <http://rdaregistry.info/Elements/e/> ;
    skos:definition "Relates an expression to an expression that is contained in or contains another expression."@en .

<http://rdaregistry.info/Elements/e/P20279> a rdf:Property ;
    rdfs:label "has on-screen participant"@en ;
    rdakit:instructionNumber "18.5" ;
    rdakit:seeAlso <http://rdaregistry.info/Elements/e/P20013> ;
    rdakit:toolkitDefinition "An agent contributing to an expression of a nonfiction moving image work by taking an active role as a participant."@en,
        "Una persona, familia o entidad corporativa que contribuye a una expresión de una obra de no ficción de imagen en movimiento mediante la adopción de un papel activo como participante."@es ;
    rdakit:toolkitLabel "on-screen participant"@en,
        "participante en pantalla"@es ;
    reg:hasSubproperty <http://rdaregistry.info/Elements/e/object/P20279> ;
    reg:hasUnconstrained <http://rdaregistry.info/Elements/u/P60824> ;
    reg:lexicalAlias <http://rdaregistry.info/Elements/e/onScreenParticipant.en> ;
    reg:name "onScreenParticipant"@en ;
    reg:status <http://metadataregistry.org/uri/RegStatus/1001> ;
    rdfs:domain <http://rdaregistry.info/Elements/c/C10006> ;
    rdfs:isDefinedBy <http://rdaregistry.info/Elements/e/> ;
    rdfs:subPropertyOf <http://rdaregistry.info/Elements/e/P20053> ;
    skos:definition "Relates an expression to an agent contributing to an expression of a nonfiction moving image work by taking an active role as a participant."@en ;
    skos:scopeNote "Appearance on screen to provide contextual or background information is excluded."@en .

<http://rdaregistry.info/Elements/e/P20293> a rdf:Property ;
    rdfs:label "has mixing engineer"@en ;
    rdakit:instructionNumber "18.5" ;
    rdakit:seeAlso <http://rdaregistry.info/Elements/w/P10306> ;
    rdakit:toolkitDefinition "An audio engineer contributing to the audio content of an expression by manipulating, mixing, and assembling the multiple tracks of a recording."@en ;
    rdakit:toolkitLabel "mixing engineer"@en ;
    reg:hasSubproperty <http://rdaregistry.info/Elements/e/object/P20293> ;
    reg:hasUnconstrained <http://rdaregistry.info/Elements/u/P60893> ;
    reg:lexicalAlias <http://rdaregistry.info/Elements/e/mixingEngineer.en> ;
    reg:name "mixingEngineer"@en ;
    reg:status <http://metadataregistry.org/uri/RegStatus/1001> ;
    rdfs:domain <http://rdaregistry.info/Elements/c/C10006> ;
    rdfs:isDefinedBy <http://rdaregistry.info/Elements/e/> ;
    rdfs:subPropertyOf <http://rdaregistry.info/Elements/e/P20292> ;
    skos:definition "Relates an expression to an audio engineer contributing to the audio content of an expression by manipulating, mixing, and assembling the multiple tracks of a recording."@en ;
    skos:scopeNote "Remixing activities that substantially change the nature and content of the original work, resulting in a new work, are excluded."@en .

<http://rdaregistry.info/Elements/e/P20305> a rdf:Property ;
    rdfs:label "has related collective agent (expression)"@en ;
    reg:hasSubproperty <http://rdaregistry.info/Elements/e/datatype/P20305>,
        <http://rdaregistry.info/Elements/e/object/P20305> ;
    reg:lexicalAlias <http://rdaregistry.info/Elements/e/relatedCollectiveAgentExpression.en> ;
    reg:name "relatedCollectiveAgentExpression"@en ;
    reg:status <http://metadataregistry.org/uri/RegStatus/1001> ;
    rdfs:domain <http://rdaregistry.info/Elements/c/C10006> ;
    rdfs:isDefinedBy <http://rdaregistry.info/Elements/e/> ;
    rdfs:subPropertyOf <http://rdaregistry.info/Elements/e/P20301> ;
    skos:definition "Relates an expression to a collective agent associated with an expression being described."@en .

<http://rdaregistry.info/Elements/e/P20011> a rdf:Property ;
    rdfs:label "has conductor"@en ;
    rdakit:instructionNumber "18.5" ;
    rdakit:toolkitDefinition "A performer contributing to an expression of a musical work by leading a performing group in a musical or dramatic presentation, etc."@en,
        "Un intérprete que contribuye a una expresión de una obra musical dirigiendo un grupo de interpretación (orquesta, coro, ópera, etc.) en una presentación musical o teatral, etc."@es,
        "Interprète contribuant à une expression d’une œuvre musicale en dirigeant un groupe d’interprètes (orchestre, chorale, opéra, etc.) dans une représentation musicale ou dramatique, etc."@fr ;
    rdakit:toolkitLabel "conductor"@en,
        "director de orquesta"@es,
        "chef d’orchestre"@fr ;
    reg:hasSubproperty <http://rdaregistry.info/Elements/e/P20285>,
        <http://rdaregistry.info/Elements/e/P20286>,
        <http://rdaregistry.info/Elements/e/object/P20011> ;
    reg:hasUnconstrained <http://rdaregistry.info/Elements/u/P60141> ;
    reg:lexicalAlias <http://rdaregistry.info/Elements/e/conductor.en> ;
    reg:name "conductor"@en ;
    reg:status <http://metadataregistry.org/uri/RegStatus/1001> ;
    rdfs:domain <http://rdaregistry.info/Elements/c/C10006> ;
    rdfs:isDefinedBy <http://rdaregistry.info/Elements/e/> ;
    rdfs:subPropertyOf <http://rdaregistry.info/Elements/e/P20039> ;
    skos:definition "Relates an expression to a performer contributing to an expression of a musical work by leading a performing group in a musical or dramatic presentation, etc."@en .

<http://rdaregistry.info/Elements/e/P20051> a rdf:Property ;
    rdfs:label "has illustrator"@en ;
    rdakit:instructionNumber "18.5" ;
    rdakit:seeAlso <http://rdaregistry.info/Elements/w/P10058> ;
    rdakit:toolkitDefinition "An agent contributing to an expression of a work by supplementing the primary content with drawings, diagrams, photographs, etc."@en,
        "Una persona, familia o entidad corporativa que contribuye a una expresión de una obra complementando el contenido primario con dibujos, diagramas, fotografías, etc."@es,
        "Personne, famille ou collectivité contribuant à une expression d’une œuvre en complétant le contenu principal avec des dessins, des diagrammes, des photographies, etc."@fr ;
    rdakit:toolkitLabel "illustrator"@en,
        "ilustrador"@es,
        "illustrateur"@fr ;
    reg:hasSubproperty <http://rdaregistry.info/Elements/e/P20259>,
        <http://rdaregistry.info/Elements/e/P20288>,
        <http://rdaregistry.info/Elements/e/object/P20051> ;
    reg:hasUnconstrained <http://rdaregistry.info/Elements/u/P60396> ;
    reg:lexicalAlias <http://rdaregistry.info/Elements/e/illustrator.en> ;
    reg:name "illustrator"@en ;
    reg:status <http://metadataregistry.org/uri/RegStatus/1001> ;
    rdfs:domain <http://rdaregistry.info/Elements/c/C10006> ;
    rdfs:isDefinedBy <http://rdaregistry.info/Elements/e/> ;
    rdfs:subPropertyOf <http://rdaregistry.info/Elements/e/P20053> ;
    skos:definition "Relates an expression to an agent contributing to an expression of a work by supplementing the primary content with drawings, diagrams, photographs, etc."@en ;
    skos:scopeNote "Creation of content that is primarily artistic is excluded."@en .

<http://rdaregistry.info/Elements/e/P20234> a rdf:Property ;
    reg:hasSubproperty <http://rdaregistry.info/Elements/e/P20072>,
        <http://rdaregistry.info/Elements/e/P20202> ;
    reg:status <http://metadataregistry.org/uri/RegStatus/1008> ;
    rdfs:isDefinedBy <http://rdaregistry.info/Elements/e/> ;
    rdfs:subPropertyOf <http://rdaregistry.info/Elements/e/P20205> .

<http://rdaregistry.info/Elements/e/P20292> a rdf:Property ;
    rdfs:label "has audio engineer"@en ;
    rdakit:instructionNumber "18.5" ;
    rdakit:toolkitDefinition "An agent contributing to the audio content of an expression by managing the technical aspects of sound during the processes of recording, mixing, and reproduction."@en ;
    rdakit:toolkitLabel "audio engineer"@en ;
    reg:hasSubproperty <http://rdaregistry.info/Elements/e/P20293>,
        <http://rdaregistry.info/Elements/e/object/P20292> ;
    reg:hasUnconstrained <http://rdaregistry.info/Elements/u/P60892> ;
    reg:lexicalAlias <http://rdaregistry.info/Elements/e/audioEngineer.en> ;
    reg:name "audioEngineer"@en ;
    reg:status <http://metadataregistry.org/uri/RegStatus/1001> ;
    rdfs:domain <http://rdaregistry.info/Elements/c/C10006> ;
    rdfs:isDefinedBy <http://rdaregistry.info/Elements/e/> ;
    rdfs:subPropertyOf <http://rdaregistry.info/Elements/e/P20053> ;
    skos:definition "Relates an expression to an agent contributing to the audio content of an expression by managing the technical aspects of sound during the processes of recording, mixing, and reproduction."@en .

<http://rdaregistry.info/Elements/e/P20301> a rdf:Property ;
    rdfs:label "has related agent (expression)"@en ;
    reg:hasSubproperty <http://rdaregistry.info/Elements/e/datatype/P20301>,
        <http://rdaregistry.info/Elements/e/object/P20301> ;
    reg:lexicalAlias <http://rdaregistry.info/Elements/e/relatedAgentExpression.en> ;
    reg:name "relatedAgentExpression"@en ;
    reg:status <http://metadataregistry.org/uri/RegStatus/1001> ;
    rdfs:domain <http://rdaregistry.info/Elements/c/C10006> ;
    rdfs:isDefinedBy <http://rdaregistry.info/Elements/e/> ;
    rdfs:subPropertyOf <http://rdaregistry.info/Elements/e/P20297> ;
    skos:definition "Relates an expression to an agent associated with an expression being described."@en .

<http://rdaregistry.info/Elements/e/P20062> a rdf:Property ;
    rdfs:label "has form of notation"@en,
        "har form av notation"@sv ;
    rdakit:instructionNumber "7.13" ;
    rdakit:toolkitDefinition "A set of characters or symbols used to express the content of an expression."@en,
        "Un conjunto de caracteres y/o símbolos utilizados para expresar el contenido de un recurso."@es,
        "Ensemble de signes et/ou de symboles utilisés pour exprimer le contenu d’une ressource."@fr ;
    rdakit:toolkitLabel "form of notation"@en,
        "forma de notación"@es,
        "forme de la notation"@fr,
        "form av notation"@sv ;
    reg:hasSubproperty <http://rdaregistry.info/Elements/e/P20061>,
        <http://rdaregistry.info/Elements/e/P20063>,
        <http://rdaregistry.info/Elements/e/P20064>,
        <http://rdaregistry.info/Elements/e/P20065> ;
    reg:hasUnconstrained <http://rdaregistry.info/Elements/u/P60319> ;
    reg:lexicalAlias <http://rdaregistry.info/Elements/e/formOfNotation.en> ;
    reg:name "formOfNotation"@en ;
    reg:status <http://metadataregistry.org/uri/RegStatus/1001> ;
    rdfs:domain <http://rdaregistry.info/Elements/c/C10006> ;
    rdfs:isDefinedBy <http://rdaregistry.info/Elements/e/> ;
    skos:definition "Relates an expression to a set of characters or symbols used to express the content of an expression."@en .

<http://rdaregistry.info/Elements/e/P20096> a rdf:Property ;
    rdfs:label "is adapted as screenplay (expression)"@en ;
    rdakit:instructionNumber "24.5" ;
    rdakit:toolkitDefinition "An expression of a work consisting of a screenplay for a motion picture, television program, or video, based on a source work."@en,
        "Una expresión de una obra que consiste en el guión para una película cinematográfica, programa de televisión o video, basado en la obra fuente."@es,
        "Expression d’une œuvre consistant en le scénario pour un film, une émission de télévision ou une vidéo, basée sur l’œuvre source."@fr ;
    rdakit:toolkitLabel "adapted as screenplay (expression)"@en,
        "adaptada como guión (expresión)"@es,
        "adapté en scénario (expression)"@fr ;
    reg:hasSubproperty <http://rdaregistry.info/Elements/e/P20095>,
        <http://rdaregistry.info/Elements/e/P20097>,
        <http://rdaregistry.info/Elements/e/P20098>,
        <http://rdaregistry.info/Elements/e/object/P20096> ;
    reg:hasUnconstrained <http://rdaregistry.info/Elements/u/P60185> ;
    reg:lexicalAlias <http://rdaregistry.info/Elements/e/adaptedAsScreenplayExpression.en> ;
    reg:name "adaptedAsScreenplayExpression"@en ;
    reg:status <http://metadataregistry.org/uri/RegStatus/1001> ;
    rdfs:domain <http://rdaregistry.info/Elements/c/C10006> ;
    rdfs:isDefinedBy <http://rdaregistry.info/Elements/e/> ;
    rdfs:subPropertyOf <http://rdaregistry.info/Elements/e/P20153> ;
    skos:definition "Relates an expression to an expression of a work consisting of a screenplay for a motion picture, television program, or video, based on a source work."@en .

<http://rdaregistry.info/Elements/e/P20102> a rdf:Property ;
    rdfs:label "is screenplay for (expression)"@en ;
    rdakit:instructionNumber "24.5" ;
    rdakit:toolkitDefinition "An expression of a work such as a motion picture, television program, or video, that uses the text of a work as a screenplay."@en,
        "Una expresión de una obra tal como una película cinematográfica, programa de televisión o video, que utiliza el texto de la obra como un guión cinematográfico."@es,
        "Expression d’une œuvre telle qu’un film, une émission de télévision ou une vidéo qui utilise le texte de l’œuvre comme scénario."@fr ;
    rdakit:toolkitLabel "screenplay for (expression)"@en,
        "guión para (expresión)"@es,
        "scénario pour (expression)"@fr ;
    reg:hasSubproperty <http://rdaregistry.info/Elements/e/P20173>,
        <http://rdaregistry.info/Elements/e/P20174>,
        <http://rdaregistry.info/Elements/e/P20175>,
        <http://rdaregistry.info/Elements/e/object/P20102> ;
    reg:hasUnconstrained <http://rdaregistry.info/Elements/u/P60201> ;
    reg:lexicalAlias <http://rdaregistry.info/Elements/e/screenplayForExpression.en> ;
    reg:name "screenplayForExpression"@en ;
    reg:status <http://metadataregistry.org/uri/RegStatus/1001> ;
    rdfs:domain <http://rdaregistry.info/Elements/c/C10006> ;
    rdfs:isDefinedBy <http://rdaregistry.info/Elements/e/> ;
    rdfs:subPropertyOf <http://rdaregistry.info/Elements/e/P20100> ;
    skos:definition "Relates an expression to an expression of a work such as a motion picture, television program, or video, that uses the text of a work as a screenplay."@en .

<http://rdaregistry.info/Elements/e/P20129> a rdf:Property ;
    rdfs:label "is screenplay based on (expression)"@en ;
    rdakit:instructionNumber "24.5" ;
    rdakit:toolkitDefinition "An expression of a work that has been adapted as a screenplay for a motion picture, television program, or video."@en,
        "Una expresión de una obra que fue adaptada como guión para una película cinematográfica, programa de televisión o vídeo."@es,
        "Expression d’une œuvre qui a été adaptée en scénario pour un film, une émission de télévision ou une vidéo."@fr ;
    rdakit:toolkitLabel "screenplay based on (expression)"@en,
        "guión basado en (expresión)"@es,
        "scénario basé sur (expression)"@fr ;
    reg:hasSubproperty <http://rdaregistry.info/Elements/e/P20130>,
        <http://rdaregistry.info/Elements/e/P20131>,
        <http://rdaregistry.info/Elements/e/P20132>,
        <http://rdaregistry.info/Elements/e/object/P20129> ;
    reg:hasUnconstrained <http://rdaregistry.info/Elements/u/P60231> ;
    reg:lexicalAlias <http://rdaregistry.info/Elements/e/screenplayBasedOnExpression.en> ;
    reg:name "screenplayBasedOnExpression"@en ;
    reg:status <http://metadataregistry.org/uri/RegStatus/1001> ;
    rdfs:domain <http://rdaregistry.info/Elements/c/C10006> ;
    rdfs:isDefinedBy <http://rdaregistry.info/Elements/e/> ;
    rdfs:subPropertyOf <http://rdaregistry.info/Elements/e/P20152> ;
    skos:definition "Relates an expression to an expression of a work that has been adapted as a screenplay for a motion picture, television program, or video."@en .

<http://rdaregistry.info/Elements/e/P20157> a rdf:Property ;
    rdfs:label "is screenplay (expression)"@en ;
    rdakit:instructionNumber "24.5" ;
    rdakit:toolkitDefinition "An expression of a work that provides text for a motion picture, television program or video."@en,
        "Una expresión de una obra que proporciona el texto para una película cinematográfica, programa de televisión o video."@es,
        "Expression d’une œuvre qui fournit le texte d’un film, d’une émission de télévision ou d’une vidéo."@fr ;
    rdakit:toolkitLabel "screenplay (expression)"@en,
        "guión (expresión)"@es,
        "scénario (expression)"@fr ;
    reg:hasSubproperty <http://rdaregistry.info/Elements/e/P20158>,
        <http://rdaregistry.info/Elements/e/P20161>,
        <http://rdaregistry.info/Elements/e/P20162>,
        <http://rdaregistry.info/Elements/e/object/P20157> ;
    reg:hasUnconstrained <http://rdaregistry.info/Elements/u/P60264> ;
    reg:lexicalAlias <http://rdaregistry.info/Elements/e/screenplayExpression.en> ;
    reg:name "screenplayExpression"@en ;
    reg:status <http://metadataregistry.org/uri/RegStatus/1001> ;
    rdfs:domain <http://rdaregistry.info/Elements/c/C10006> ;
    rdfs:isDefinedBy <http://rdaregistry.info/Elements/e/> ;
    rdfs:subPropertyOf <http://rdaregistry.info/Elements/e/P20100> ;
    skos:definition "Relates an expression to an expression of a work that provides text for a motion picture, television program or video."@en .

<http://rdaregistry.info/Elements/e/P20224> a rdf:Property ;
    rdfs:label "has colour content"@en,
        "har färginnehåll"@sv ;
    rdakit:instructionNumber "7.17" ;
    rdakit:toolkitDefinition "A presence of colour, tone, etc., in the content of an expression."@en,
        "La presencia de color, tono, etc., en el contenido de un recurso."@es,
        "La présence de couleur, teinte, etc. dans le contenu d’une ressource."@fr ;
    rdakit:toolkitLabel "colour content"@en,
        "contenido a color"@es,
        "contenu de couleur"@fr,
        "färginnehåll"@sv ;
    reg:hasSubproperty <http://rdaregistry.info/Elements/e/P20220>,
        <http://rdaregistry.info/Elements/e/P20221>,
        <http://rdaregistry.info/Elements/e/P20222>,
        <http://rdaregistry.info/Elements/e/P20223> ;
    reg:hasUnconstrained <http://rdaregistry.info/Elements/u/P60558> ;
    reg:lexicalAlias <http://rdaregistry.info/Elements/e/colourContent.en> ;
    reg:name "colourContent"@en ;
    reg:status <http://metadataregistry.org/uri/RegStatus/1001> ;
    rdfs:domain <http://rdaregistry.info/Elements/c/C10006> ;
    rdfs:isDefinedBy <http://rdaregistry.info/Elements/e/> ;
    skos:definition "Relates an expression to a presence of colour, tone, etc., in the content of an expression."@en ;
    skos:scopeNote "Black, white, single colour shades of black, single colour tints of white, and single colour tones of gray are considered to be single colours."@en .

<http://rdaregistry.info/Elements/e/P20228> a rdf:Property ;
    rdfs:label "has scale"@en,
        "har skala"@sv ;
    rdakit:instructionNumber "7.25" ;
    rdakit:toolkitDefinition "A ratio of the dimensions of the content of an image or three-dimensional form to the dimensions of the thing that is represented."@en,
        "La proporción de las dimensiones de una imagen o forma tridimensional incluida o incorporada en un recurso con las dimensiones de la entidad que representa."@es,
        "Le rapport entre les dimensions d’une image ou d’une forme tridimensionnelle, contenue ou matérialisée dans une ressource, et les dimensions de l’entité qu’elle représente."@fr ;
    rdakit:toolkitLabel "scale"@en,
        "escala"@es,
        "échelle"@fr,
        "skala"@sv ;
    reg:hasSubproperty <http://rdaregistry.info/Elements/e/P20213>,
        <http://rdaregistry.info/Elements/e/P20226>,
        <http://rdaregistry.info/Elements/e/P20227>,
        <http://rdaregistry.info/Elements/e/P20230> ;
    reg:hasUnconstrained <http://rdaregistry.info/Elements/u/P60565> ;
    reg:lexicalAlias <http://rdaregistry.info/Elements/e/scale.en> ;
    reg:name "scale"@en ;
    reg:status <http://metadataregistry.org/uri/RegStatus/1001> ;
    rdfs:domain <http://rdaregistry.info/Elements/c/C10006> ;
    rdfs:isDefinedBy <http://rdaregistry.info/Elements/e/> ;
    skos:definition "Relates an expression to a ratio of the dimensions of the content of an image or three-dimensional form to the dimensions of the thing that is represented."@en ;
    skos:scopeNote "Scale can apply to horizontal, vertical, angular, and/or other measurements represented in an expression."@en .

<http://rdaregistry.info/Elements/e/P20232> a rdf:Property ;
    rdfs:label "has accompanying expression relationship with"@en ;
    rdakit:instructionNumber "24.5" ;
    rdakit:toolkitDefinition "An expression of a work that is an augmentation of, or is augmented by, or is complemented by another expression."@en,
        "Una expresión de una obra que es un aumento de, o se ve aumentada por, o se complementa con la expresión."@es,
        "Expression d’une œuvre qui constitue une augmentation de l’expression ou qui est augmentée ou complétée par elle."@fr ;
    rdakit:toolkitLabel "accompanying expression relationship"@en,
        "relaciones de expresión acompañante"@es,
        "relation d’expression d’accompagnement"@fr ;
    reg:hasSubproperty <http://rdaregistry.info/Elements/e/P20100>,
        <http://rdaregistry.info/Elements/e/P20105>,
        <http://rdaregistry.info/Elements/e/P20192>,
        <http://rdaregistry.info/Elements/e/object/P20232> ;
    reg:hasUnconstrained <http://rdaregistry.info/Elements/u/P60709> ;
    reg:lexicalAlias <http://rdaregistry.info/Elements/e/accompanyingExpressionRelationship.en> ;
    reg:name "accompanyingExpressionRelationship"@en ;
    reg:status <http://metadataregistry.org/uri/RegStatus/1001> ;
    rdfs:domain <http://rdaregistry.info/Elements/c/C10006> ;
    rdfs:isDefinedBy <http://rdaregistry.info/Elements/e/> ;
    rdfs:subPropertyOf <http://rdaregistry.info/Elements/e/P20205> ;
    skos:definition "Relates an expression to an expression of a work that is an augmentation of, or is augmented by, or is complemented by another expression."@en .

<http://rdaregistry.info/Elements/e/P20243> a rdf:Property ;
    rdfs:label "is music (expression)"@en ;
    rdakit:instructionNumber "24.5" ;
    rdakit:toolkitDefinition "An expression of a musical work that is used in a motion picture, play, television program, etc."@en,
        "Una expresión de una obra musical que se usa en una película cinematográfica, obra de teatro, programa de televisión, etc."@es,
        "Expression d’une œuvre musicale utilisée dans un film, une pièce de théâtre, une émission de télévision, etc."@fr ;
    rdakit:toolkitLabel "music (expression)"@en,
        "música (expresión)"@es,
        "musique (expression)"@fr ;
    reg:hasSubproperty <http://rdaregistry.info/Elements/e/P20085>,
        <http://rdaregistry.info/Elements/e/object/P20243> ;
    reg:hasUnconstrained <http://rdaregistry.info/Elements/u/P60723> ;
    reg:lexicalAlias <http://rdaregistry.info/Elements/e/musicExpression.en> ;
    reg:name "musicExpression"@en ;
    reg:status <http://metadataregistry.org/uri/RegStatus/1001> ;
    rdfs:domain <http://rdaregistry.info/Elements/c/C10006> ;
    rdfs:isDefinedBy <http://rdaregistry.info/Elements/e/> ;
    rdfs:subPropertyOf <http://rdaregistry.info/Elements/e/P20100> ;
    skos:definition "Relates an expression to an expression of a musical work that is used in a motion picture, play, television program, etc."@en .

<http://rdaregistry.info/Elements/e/P20244> a rdf:Property ;
    rdfs:label "is music for (expression)"@en ;
    rdakit:instructionNumber "24.5" ;
    rdakit:toolkitDefinition "An expression of a work such as a motion picture, play, television program, etc. that uses a musical work."@en,
        "Una expresión de una obra tal como una película cinematográfica, obra de teatro, programa de televisión, etc., que usa una obra musical."@es,
        "Expression d’une œuvre telle qu’un film, une pièce de théâtre, une émission de télévision, etc. qui utilise l’œuvre musicale."@fr ;
    rdakit:toolkitLabel "music for (expression)"@en,
        "música de (expresión)"@es,
        "musique pour (expression)"@fr ;
    reg:hasSubproperty <http://rdaregistry.info/Elements/e/P20103>,
        <http://rdaregistry.info/Elements/e/object/P20244> ;
    reg:hasUnconstrained <http://rdaregistry.info/Elements/u/P60724> ;
    reg:lexicalAlias <http://rdaregistry.info/Elements/e/musicForExpression.en> ;
    reg:name "musicForExpression"@en ;
    reg:status <http://metadataregistry.org/uri/RegStatus/1001> ;
    rdfs:domain <http://rdaregistry.info/Elements/c/C10006> ;
    rdfs:isDefinedBy <http://rdaregistry.info/Elements/e/> ;
    rdfs:subPropertyOf <http://rdaregistry.info/Elements/e/P20100> ;
    skos:definition "Relates an expression to an expression of a work such as a motion picture, play, television program, etc., that uses a musical work."@en .

<http://rdaregistry.info/Elements/e/P20072> a rdf:Property ;
    reg:hasSubproperty <http://rdaregistry.info/Elements/e/P20136>,
        <http://rdaregistry.info/Elements/e/P20150>,
        <http://rdaregistry.info/Elements/e/P20178>,
        <http://rdaregistry.info/Elements/e/P20182>,
        <http://rdaregistry.info/Elements/e/P20187> ;
    reg:status <http://metadataregistry.org/uri/RegStatus/1008> ;
    rdfs:isDefinedBy <http://rdaregistry.info/Elements/e/> ;
    rdfs:subPropertyOf <http://rdaregistry.info/Elements/e/P20234> .

<http://rdaregistry.info/Elements/e/P20202> a rdf:Property ;
    reg:hasSubproperty <http://rdaregistry.info/Elements/e/P20111>,
        <http://rdaregistry.info/Elements/e/P20112>,
        <http://rdaregistry.info/Elements/e/P20113>,
        <http://rdaregistry.info/Elements/e/P20116>,
        <http://rdaregistry.info/Elements/e/P20117> ;
    reg:status <http://metadataregistry.org/uri/RegStatus/1008> ;
    rdfs:isDefinedBy <http://rdaregistry.info/Elements/e/> ;
    rdfs:subPropertyOf <http://rdaregistry.info/Elements/e/P20234> .

<http://rdaregistry.info/Elements/e/P20269> a rdf:Property ;
    rdfs:label "is described in (expression)"@en ;
    rdakit:instructionNumber "23.5" ;
    rdakit:toolkitDefinition "A work that describes a described expression."@en,
        "Una obra que describe una expresión descrita."@es,
        "Expression d’une œuvre qui décrit une expression."@fr ;
    rdakit:toolkitLabel "described in (expression)"@en,
        "descrita en (expresión)"@es,
        "décrit dans (expression)"@fr ;
    reg:hasSubproperty <http://rdaregistry.info/Elements/e/P20270>,
        <http://rdaregistry.info/Elements/e/P20271>,
        <http://rdaregistry.info/Elements/e/P20272>,
        <http://rdaregistry.info/Elements/e/P20273>,
        <http://rdaregistry.info/Elements/e/P20274>,
        <http://rdaregistry.info/Elements/e/object/P20269> ;
    reg:hasUnconstrained <http://rdaregistry.info/Elements/u/P60215> ;
    reg:lexicalAlias <http://rdaregistry.info/Elements/e/describedInExpression.en> ;
    reg:name "describedInExpression"@en ;
    reg:status <http://metadataregistry.org/uri/RegStatus/1001> ;
    rdfs:domain <http://rdaregistry.info/Elements/c/C10006> ;
    rdfs:isDefinedBy <http://rdaregistry.info/Elements/e/> ;
    rdfs:subPropertyOf <http://rdaregistry.info/Elements/e/P20268> ;
    skos:definition "Relates an expression to a work that describes a described expression."@en .

<http://rdaregistry.info/Elements/e/P20046> a rdf:Property ;
    rdfs:label "has writer of supplementary textual content"@en ;
    rdakit:instructionNumber "18.5" ;
    rdakit:toolkitDefinition "An agent contributing to an expression of a work by providing supplementary textual content, such as an introduction or a preface, to an original work."@en,
        "Una persona, familia o entidad corporativa que contribuye a una expresión de una obra ofreciendo contenido textual suplementario (por ej., una introducción, un prefacio) a la obra original."@es,
        "Personne, famille ou collectivité contribuant à une expression d’une œuvre en fournissant du contenu textuel supplémentaire (par exemple, une introduction, une préface) à l’œuvre originale."@fr ;
    rdakit:toolkitLabel "writer of supplementary textual content"@en,
        "autor de contenido textual suplementario"@es,
        "auteur de contenu textuel supplémentaire"@fr ;
    reg:hasSubproperty <http://rdaregistry.info/Elements/e/P20030>,
        <http://rdaregistry.info/Elements/e/P20041>,
        <http://rdaregistry.info/Elements/e/P20044>,
        <http://rdaregistry.info/Elements/e/P20045>,
        <http://rdaregistry.info/Elements/e/P20275>,
        <http://rdaregistry.info/Elements/e/object/P20046> ;
    reg:hasUnconstrained <http://rdaregistry.info/Elements/u/P60392> ;
    reg:lexicalAlias <http://rdaregistry.info/Elements/e/writerOfSupplementaryTextualContent.en> ;
    reg:name "writerOfSupplementaryTextualContent"@en ;
    reg:status <http://metadataregistry.org/uri/RegStatus/1001> ;
    rdfs:domain <http://rdaregistry.info/Elements/c/C10006> ;
    rdfs:isDefinedBy <http://rdaregistry.info/Elements/e/> ;
    rdfs:subPropertyOf <http://rdaregistry.info/Elements/e/P20053> ;
    skos:definition "Relates an expression to an agent contributing to an expression of a work by providing supplementary textual content, such as an introduction or a preface, to an original work."@en .

<http://rdaregistry.info/Elements/e/P20297> a rdf:Property ;
    rdfs:label "has related entity (expression)"@en ;
    reg:hasSubproperty <http://rdaregistry.info/Elements/e/datatype/P20297>,
        <http://rdaregistry.info/Elements/e/object/P20297> ;
    reg:lexicalAlias <http://rdaregistry.info/Elements/e/relatedEntityExpression.en> ;
    reg:name "relatedEntityExpression"@en ;
    reg:status <http://metadataregistry.org/uri/RegStatus/1001> ;
    rdfs:domain <http://rdaregistry.info/Elements/c/C10006> ;
    rdfs:isDefinedBy <http://rdaregistry.info/Elements/e/> ;
    rdfs:subPropertyOf <http://rdaregistry.info/Elements/x/P00001> ;
    skos:definition "Relates an expression to an entity associated with an expression being described."@en .

<http://rdaregistry.info/Elements/e/P20154> a rdf:Property ;
    rdfs:label "is preceded by (expression)"@en ;
    rdakit:instructionNumber "24.5" ;
    rdakit:toolkitDefinition "An expression of a work that precedes, that is, is earlier in time or before in narrative, etc., a succeeding expression."@en,
        "Una expresión de una obra que precede (por ej., es anterior en el tiempo o en la narración) la expresión que sigue."@es,
        "Expression d’une œuvre qui précède l’expression suivante (par exemple, qui lui est antérieure dans le temps ou dans un récit)."@fr ;
    rdakit:toolkitLabel "preceded by (expression)"@en,
        "precedida por (expresión)"@es,
        "précédé de (expression)"@fr ;
    reg:hasSubproperty <http://rdaregistry.info/Elements/e/P20137>,
        <http://rdaregistry.info/Elements/e/P20138>,
        <http://rdaregistry.info/Elements/e/P20149>,
        <http://rdaregistry.info/Elements/e/P20167>,
        <http://rdaregistry.info/Elements/e/P20168>,
        <http://rdaregistry.info/Elements/e/P20198>,
        <http://rdaregistry.info/Elements/e/P20199>,
        <http://rdaregistry.info/Elements/e/P20201>,
        <http://rdaregistry.info/Elements/e/object/P20154> ;
    reg:hasUnconstrained <http://rdaregistry.info/Elements/u/P60261> ;
    reg:lexicalAlias <http://rdaregistry.info/Elements/e/precededByExpression.en> ;
    reg:name "precededByExpression"@en ;
    reg:status <http://metadataregistry.org/uri/RegStatus/1001> ;
    rdfs:domain <http://rdaregistry.info/Elements/c/C10006> ;
    rdfs:isDefinedBy <http://rdaregistry.info/Elements/e/> ;
    rdfs:subPropertyOf <http://rdaregistry.info/Elements/e/P20235> ;
    skos:definition "Relates an expression to an expression of a work that precedes, that is, is earlier in time or before in narrative, etc., a succeeding expression."@en .

<http://rdaregistry.info/Elements/e/P20169> a rdf:Property ;
    rdfs:label "is succeeded by (expression)"@en ;
    rdakit:instructionNumber "24.5" ;
    rdakit:toolkitDefinition "An expression of a work that succeeds, that is, is later in time or after in a narrative, etc., a preceding expression."@en,
        "Una expresión de una obra que sucede a (por ej., posterior en el tiempo o posterior en una narración) la expresión predecesora."@es,
        "Expression d’une œuvre qui succède à l’expression précédente (par exemple, qui lui est ultérieure dans le temps ou dans un récit)."@fr ;
    rdakit:toolkitLabel "succeeded by (expression)"@en,
        "seguida por (expresión)"@es,
        "suivi de (expression)"@fr ;
    reg:hasSubproperty <http://rdaregistry.info/Elements/e/P20075>,
        <http://rdaregistry.info/Elements/e/P20076>,
        <http://rdaregistry.info/Elements/e/P20101>,
        <http://rdaregistry.info/Elements/e/P20143>,
        <http://rdaregistry.info/Elements/e/P20144>,
        <http://rdaregistry.info/Elements/e/P20191>,
        <http://rdaregistry.info/Elements/e/P20200>,
        <http://rdaregistry.info/Elements/e/P20212>,
        <http://rdaregistry.info/Elements/e/object/P20169> ;
    reg:hasUnconstrained <http://rdaregistry.info/Elements/u/P60278> ;
    reg:lexicalAlias <http://rdaregistry.info/Elements/e/succeededByExpression.en> ;
    reg:name "succeededByExpression"@en ;
    reg:status <http://metadataregistry.org/uri/RegStatus/1001> ;
    rdfs:domain <http://rdaregistry.info/Elements/c/C10006> ;
    rdfs:isDefinedBy <http://rdaregistry.info/Elements/e/> ;
    rdfs:subPropertyOf <http://rdaregistry.info/Elements/e/P20235> ;
    skos:definition "Relates an expression to an expression of a work that succeeds, that is, is later in time or after in a narrative, etc., a preceding expression."@en .

<http://rdaregistry.info/Elements/e/P20100> a rdf:Property ;
    rdfs:label "is complemented by (expression)"@en ;
    rdakit:instructionNumber "24.5" ;
    rdakit:toolkitDefinition "An expression of a work paired with another expression without either expression being considered to predominate."@en,
        "Una expresión de una obra unida con otra entidad sin que ninguna pueda ser considerada como principal"@es,
        "Expression d’une œuvre appariée à une autre expression sans qu’aucune des deux expressions ne soit considérée comme prédominante."@fr ;
    rdakit:toolkitLabel "complemented by (expression)"@en,
        "complementada por (expresión)"@es,
        "complété par (expression)"@fr ;
    reg:hasSubproperty <http://rdaregistry.info/Elements/e/P20084>,
        <http://rdaregistry.info/Elements/e/P20102>,
        <http://rdaregistry.info/Elements/e/P20157>,
        <http://rdaregistry.info/Elements/e/P20160>,
        <http://rdaregistry.info/Elements/e/P20163>,
        <http://rdaregistry.info/Elements/e/P20176>,
        <http://rdaregistry.info/Elements/e/P20253>,
        <http://rdaregistry.info/Elements/e/P20254>,
        <http://rdaregistry.info/Elements/e/object/P20100> ;
    reg:hasUnconstrained <http://rdaregistry.info/Elements/u/P60198> ;
    reg:lexicalAlias <http://rdaregistry.info/Elements/e/complementedByExpression.en> ;
    reg:name "complementedByExpression"@en ;
    reg:status <http://metadataregistry.org/uri/RegStatus/1001> ;
    rdfs:domain <http://rdaregistry.info/Elements/c/C10006> ;
    rdfs:isDefinedBy <http://rdaregistry.info/Elements/e/> ;
    rdfs:subPropertyOf <http://rdaregistry.info/Elements/e/P20232> ;
    skos:definition "Relates an expression to an expression of a work paired with another expression without either expression being considered to predominate."@en .

<http://rdaregistry.info/Elements/e/P20105> a rdf:Property ;
    rdfs:label "is augmented by (expression)"@en ;
    rdakit:instructionNumber "24.5" ;
    rdakit:toolkitDefinition "An expression of a work that adds to the content of a predominant expression."@en,
        "Una expresión de una obra que añade al contenido de una expresión principal."@es,
        "Expression d’une œuvre qui ajoute au contenu d’une expression prédominante."@fr ;
    rdakit:toolkitLabel "augmented by (expression)"@en,
        "aumentada por (expresión)"@es,
        "augmenté par (expression)"@fr ;
    reg:hasSubproperty <http://rdaregistry.info/Elements/e/P20080>,
        <http://rdaregistry.info/Elements/e/P20093>,
        <http://rdaregistry.info/Elements/e/P20094>,
        <http://rdaregistry.info/Elements/e/P20107>,
        <http://rdaregistry.info/Elements/e/P20108>,
        <http://rdaregistry.info/Elements/e/P20109>,
        <http://rdaregistry.info/Elements/e/P20118>,
        <http://rdaregistry.info/Elements/e/P20120>,
        <http://rdaregistry.info/Elements/e/P20155>,
        <http://rdaregistry.info/Elements/e/P20156>,
        <http://rdaregistry.info/Elements/e/P20172>,
        <http://rdaregistry.info/Elements/e/object/P20105> ;
    reg:hasUnconstrained <http://rdaregistry.info/Elements/u/P60204> ;
    reg:lexicalAlias <http://rdaregistry.info/Elements/e/augmentedByExpression.en> ;
    reg:name "augmentedByExpression"@en ;
    reg:status <http://metadataregistry.org/uri/RegStatus/1001> ;
    rdfs:domain <http://rdaregistry.info/Elements/c/C10006> ;
    rdfs:isDefinedBy <http://rdaregistry.info/Elements/e/> ;
    rdfs:subPropertyOf <http://rdaregistry.info/Elements/e/P20232> ;
    skos:definition "Relates an expression to an expression of a work that adds to the content of a predominant expression."@en .

<http://rdaregistry.info/Elements/e/P20192> a rdf:Property ;
    rdfs:label "is augmentation of (expression)"@en ;
    rdakit:instructionNumber "24.5" ;
    rdakit:toolkitDefinition "An expression of a work whose content is added to by another expression."@en,
        "Una expresión de una obra cuyo contenido es añadido por otra expresión."@es,
        "Expression d’une œuvre dont le contenu est accru par une autre expression."@fr ;
    rdakit:toolkitLabel "augmentation of (expression)"@en,
        "aumento de (expresión)"@es,
        "augmentation de (expression)"@fr ;
    reg:hasSubproperty <http://rdaregistry.info/Elements/e/P20083>,
        <http://rdaregistry.info/Elements/e/P20089>,
        <http://rdaregistry.info/Elements/e/P20146>,
        <http://rdaregistry.info/Elements/e/P20147>,
        <http://rdaregistry.info/Elements/e/P20148>,
        <http://rdaregistry.info/Elements/e/P20151>,
        <http://rdaregistry.info/Elements/e/P20177>,
        <http://rdaregistry.info/Elements/e/P20180>,
        <http://rdaregistry.info/Elements/e/P20181>,
        <http://rdaregistry.info/Elements/e/P20188>,
        <http://rdaregistry.info/Elements/e/P20197>,
        <http://rdaregistry.info/Elements/e/object/P20192> ;
    reg:hasUnconstrained <http://rdaregistry.info/Elements/u/P60307> ;
    reg:lexicalAlias <http://rdaregistry.info/Elements/e/augmentationOfExpression.en> ;
    reg:name "augmentationOfExpression"@en ;
    reg:status <http://metadataregistry.org/uri/RegStatus/1001> ;
    rdfs:domain <http://rdaregistry.info/Elements/c/C10006> ;
    rdfs:isDefinedBy <http://rdaregistry.info/Elements/e/> ;
    rdfs:subPropertyOf <http://rdaregistry.info/Elements/e/P20232> ;
    skos:definition "Relates an expression to an expression of a work whose content is added to by another expression."@en .

<http://rdaregistry.info/Elements/e/P20039> a rdf:Property ;
    rdfs:label "has performer"@en ;
    rdakit:instructionNumber "18.5" ;
    rdakit:toolkitDefinition "An agent contributing to an expression of a work by performing music, acting, dancing, speaking, etc., often in a musical or dramatic presentation, etc."@en,
        "Una persona, familia o entidad corporativa que contribuye a una expresión de una obra interpretando música, actuando, danzando, hablando, etc., generalmente en una producción musical o teatral, etc."@es,
        "Personne, famille ou collectivité contribuant à une expression d’une œuvre en exécutant de la musique, en jouant, en dansant, en parlant, etc. souvent dans une représentation musicale ou dramatique, etc."@fr ;
    rdakit:toolkitLabel "performer"@en,
        "intérprete"@es,
        "interprète"@fr ;
    reg:hasSubproperty <http://rdaregistry.info/Elements/e/P20011>,
        <http://rdaregistry.info/Elements/e/P20012>,
        <http://rdaregistry.info/Elements/e/P20013>,
        <http://rdaregistry.info/Elements/e/P20014>,
        <http://rdaregistry.info/Elements/e/P20015>,
        <http://rdaregistry.info/Elements/e/P20016>,
        <http://rdaregistry.info/Elements/e/P20017>,
        <http://rdaregistry.info/Elements/e/P20018>,
        <http://rdaregistry.info/Elements/e/P20019>,
        <http://rdaregistry.info/Elements/e/P20020>,
        <http://rdaregistry.info/Elements/e/P20021>,
        <http://rdaregistry.info/Elements/e/P20022>,
        <http://rdaregistry.info/Elements/e/P20023>,
        <http://rdaregistry.info/Elements/e/P20024>,
        <http://rdaregistry.info/Elements/e/P20025>,
        <http://rdaregistry.info/Elements/e/object/P20039> ;
    reg:hasUnconstrained <http://rdaregistry.info/Elements/u/P60387> ;
    reg:lexicalAlias <http://rdaregistry.info/Elements/e/performer.en> ;
    reg:name "performer"@en ;
    reg:status <http://metadataregistry.org/uri/RegStatus/1001> ;
    rdfs:domain <http://rdaregistry.info/Elements/c/C10006> ;
    rdfs:isDefinedBy <http://rdaregistry.info/Elements/e/> ;
    rdfs:subPropertyOf <http://rdaregistry.info/Elements/e/P20053> ;
    skos:definition "Relates an expression to an agent contributing to an expression of a work by performing music, acting, dancing, speaking, etc., often in a musical or dramatic presentation, etc."@en .

<http://rdaregistry.info/Elements/e/P20152> a rdf:Property ;
    rdfs:label "is adaptation of (expression)"@en ;
    rdakit:instructionNumber "24.5" ;
    rdakit:toolkitDefinition "An expression of a work that has been modified for a purpose, use, or medium other than that for which it was originally intended."@en,
        "Una expresión de una obra que ha sido modificada para un propósito, uso o medio diferente del previsto originalmente."@es,
        "Expression d’une œuvre qui a été modifiée pour une fin, une utilisation ou un mode d’expression autre que celui auquel elle était destinée à l’origine."@fr ;
    rdakit:toolkitLabel "adaptation of (expression)"@en,
        "adaptación de (expresión)"@es,
        "adaptation de (expression)"@fr ;
    reg:hasSubproperty <http://rdaregistry.info/Elements/e/P20123>,
        <http://rdaregistry.info/Elements/e/P20124>,
        <http://rdaregistry.info/Elements/e/P20125>,
        <http://rdaregistry.info/Elements/e/P20126>,
        <http://rdaregistry.info/Elements/e/P20127>,
        <http://rdaregistry.info/Elements/e/P20128>,
        <http://rdaregistry.info/Elements/e/P20129>,
        <http://rdaregistry.info/Elements/e/P20133>,
        <http://rdaregistry.info/Elements/e/P20134>,
        <http://rdaregistry.info/Elements/e/P20256>,
        <http://rdaregistry.info/Elements/e/P20281>,
        <http://rdaregistry.info/Elements/e/object/P20152> ;
    reg:hasUnconstrained <http://rdaregistry.info/Elements/u/P60241> ;
    reg:lexicalAlias <http://rdaregistry.info/Elements/e/adaptationOfExpression.en> ;
    reg:name "adaptationOfExpression"@en ;
    reg:status <http://metadataregistry.org/uri/RegStatus/1001> ;
    rdfs:domain <http://rdaregistry.info/Elements/c/C10006> ;
    rdfs:isDefinedBy <http://rdaregistry.info/Elements/e/> ;
    rdfs:subPropertyOf <http://rdaregistry.info/Elements/e/P20204> ;
    skos:definition "Relates an expression to an expression of a work that has been modified for a purpose, use, or medium other than that for which it was originally intended."@en .

<http://rdaregistry.info/Elements/e/P20153> a rdf:Property ;
    rdfs:label "is adapted as (expression)"@en ;
    rdakit:instructionNumber "24.5" ;
    rdakit:toolkitDefinition "An expression of a work that modifies a source expression for a purpose, use, or medium other than that for which it was originally intended."@en,
        "Una expresión de una obra que modifica la expresión fuente para un propósito, uso o medio diferente del previsto originalmente."@es,
        "Expression d’une œuvre qui modifie l’expression source pour une fin, une utilisation ou un mode d’expression autre que celui auquel elle était destinée à l’origine."@fr ;
    rdakit:toolkitLabel "adapted as (expression)"@en,
        "adaptada como (expresión)"@es,
        "adapté comme (expression)"@fr ;
    reg:hasSubproperty <http://rdaregistry.info/Elements/e/P20009>,
        <http://rdaregistry.info/Elements/e/P20060>,
        <http://rdaregistry.info/Elements/e/P20066>,
        <http://rdaregistry.info/Elements/e/P20067>,
        <http://rdaregistry.info/Elements/e/P20073>,
        <http://rdaregistry.info/Elements/e/P20077>,
        <http://rdaregistry.info/Elements/e/P20088>,
        <http://rdaregistry.info/Elements/e/P20096>,
        <http://rdaregistry.info/Elements/e/P20099>,
        <http://rdaregistry.info/Elements/e/P20255>,
        <http://rdaregistry.info/Elements/e/P20282>,
        <http://rdaregistry.info/Elements/e/object/P20153> ;
    reg:hasUnconstrained <http://rdaregistry.info/Elements/u/P60260> ;
    reg:lexicalAlias <http://rdaregistry.info/Elements/e/adaptedAsExpression.en> ;
    reg:name "adaptedAsExpression"@en ;
    reg:status <http://metadataregistry.org/uri/RegStatus/1001> ;
    rdfs:domain <http://rdaregistry.info/Elements/c/C10006> ;
    rdfs:isDefinedBy <http://rdaregistry.info/Elements/e/> ;
    rdfs:subPropertyOf <http://rdaregistry.info/Elements/e/P20203> ;
    skos:definition "Relates an expression to an expression of a work based on a source expression."@en .

<http://rdaregistry.info/Elements/e/P20203> a rdf:Property ;
    rdfs:label "is derivative (expression)"@en ;
    rdakit:instructionNumber "24.5" ;
    rdakit:toolkitDefinition "An expression that is a modification of a source expression."@en,
        "Una expresión que es una modificación de una expresión fuente."@es,
        "Expression qui est une modification d’une expression source."@fr ;
    rdakit:toolkitLabel "derivative (expression)"@en,
        "expresión derivada"@es,
        "dérivé (expression)"@fr ;
    reg:hasSubproperty <http://rdaregistry.info/Elements/e/P20082>,
        <http://rdaregistry.info/Elements/e/P20086>,
        <http://rdaregistry.info/Elements/e/P20087>,
        <http://rdaregistry.info/Elements/e/P20090>,
        <http://rdaregistry.info/Elements/e/P20091>,
        <http://rdaregistry.info/Elements/e/P20092>,
        <http://rdaregistry.info/Elements/e/P20104>,
        <http://rdaregistry.info/Elements/e/P20106>,
        <http://rdaregistry.info/Elements/e/P20110>,
        <http://rdaregistry.info/Elements/e/P20114>,
        <http://rdaregistry.info/Elements/e/P20115>,
        <http://rdaregistry.info/Elements/e/P20119>,
        <http://rdaregistry.info/Elements/e/P20153>,
        <http://rdaregistry.info/Elements/e/P20164>,
        <http://rdaregistry.info/Elements/e/P20165>,
        <http://rdaregistry.info/Elements/e/P20166>,
        <http://rdaregistry.info/Elements/e/P20170>,
        <http://rdaregistry.info/Elements/e/P20171>,
        <http://rdaregistry.info/Elements/e/P20204>,
        <http://rdaregistry.info/Elements/e/P20211>,
        <http://rdaregistry.info/Elements/e/object/P20203> ;
    reg:hasUnconstrained <http://rdaregistry.info/Elements/u/P60250> ;
    reg:lexicalAlias <http://rdaregistry.info/Elements/e/derivativeExpression.en> ;
    reg:name "derivativeExpression"@en ;
    reg:status <http://metadataregistry.org/uri/RegStatus/1001> ;
    rdfs:domain <http://rdaregistry.info/Elements/c/C10006> ;
    rdfs:isDefinedBy <http://rdaregistry.info/Elements/e/> ;
    rdfs:subPropertyOf <http://rdaregistry.info/Elements/e/P20233> ;
    skos:definition "Relates an expression to an expression that is a modification of a source expression."@en .

<http://rdaregistry.info/Elements/e/P20204> a rdf:Property ;
    rdfs:label "is based on (expression)"@en ;
    rdakit:instructionNumber "24.5" ;
    rdakit:toolkitDefinition "An expression used as the basis for a derivative expression."@en,
        "Una expresión utilizada como base para una expresión derivada."@es,
        "Expression servant de base à une expression dérivée."@fr ;
    rdakit:toolkitLabel "based on (expression)"@en,
        "basada en (expresión)"@es,
        "basé sur (expression)"@fr ;
    reg:hasSubproperty <http://rdaregistry.info/Elements/e/P20081>,
        <http://rdaregistry.info/Elements/e/P20121>,
        <http://rdaregistry.info/Elements/e/P20122>,
        <http://rdaregistry.info/Elements/e/P20135>,
        <http://rdaregistry.info/Elements/e/P20139>,
        <http://rdaregistry.info/Elements/e/P20140>,
        <http://rdaregistry.info/Elements/e/P20141>,
        <http://rdaregistry.info/Elements/e/P20152>,
        <http://rdaregistry.info/Elements/e/P20159>,
        <http://rdaregistry.info/Elements/e/P20179>,
        <http://rdaregistry.info/Elements/e/P20183>,
        <http://rdaregistry.info/Elements/e/P20184>,
        <http://rdaregistry.info/Elements/e/P20185>,
        <http://rdaregistry.info/Elements/e/P20186>,
        <http://rdaregistry.info/Elements/e/P20189>,
        <http://rdaregistry.info/Elements/e/P20190>,
        <http://rdaregistry.info/Elements/e/P20193>,
        <http://rdaregistry.info/Elements/e/P20194>,
        <http://rdaregistry.info/Elements/e/P20195>,
        <http://rdaregistry.info/Elements/e/object/P20204> ;
    reg:hasUnconstrained <http://rdaregistry.info/Elements/u/P60305> ;
    reg:lexicalAlias <http://rdaregistry.info/Elements/e/basedOnExpression.en> ;
    reg:name "basedOnExpression"@en ;
    reg:status <http://metadataregistry.org/uri/RegStatus/1001> ;
    rdfs:domain <http://rdaregistry.info/Elements/c/C10006> ;
    rdfs:isDefinedBy <http://rdaregistry.info/Elements/e/> ;
    rdfs:subPropertyOf <http://rdaregistry.info/Elements/e/P20233> ;
    skos:definition "Relates an expression to an expression used as the basis for a derivative expression."@en .

<http://metadataregistry.org/uri/RegStatus/1008> a skos:Concept ;
    skos:prefLabel "Deprecated"@en .

<http://rdaregistry.info/Elements/e/P20053> a rdf:Property ;
    rdfs:label "has contributor"@en,
        "har bidragsgivare"@sv ;
    rdakit:instructionNumber "20.2" ;
    rdakit:toolkitDefinition "An agent contributing to an expression."@en,
        "Una persona, familia o entidad corporativa que contribuye a  una expresión."@es,
        "Personne, famille ou collectivité contribuant à une expression."@fr ;
    rdakit:toolkitLabel "contributor"@en,
        "colaborador"@es,
        "contributeur"@fr,
        "bidragsgivare"@sv ;
    reg:hasSubproperty <http://rdaregistry.info/Elements/e/P20026>,
        <http://rdaregistry.info/Elements/e/P20027>,
        <http://rdaregistry.info/Elements/e/P20028>,
        <http://rdaregistry.info/Elements/e/P20029>,
        <http://rdaregistry.info/Elements/e/P20031>,
        <http://rdaregistry.info/Elements/e/P20032>,
        <http://rdaregistry.info/Elements/e/P20033>,
        <http://rdaregistry.info/Elements/e/P20034>,
        <http://rdaregistry.info/Elements/e/P20035>,
        <http://rdaregistry.info/Elements/e/P20036>,
        <http://rdaregistry.info/Elements/e/P20037>,
        <http://rdaregistry.info/Elements/e/P20038>,
        <http://rdaregistry.info/Elements/e/P20039>,
        <http://rdaregistry.info/Elements/e/P20040>,
        <http://rdaregistry.info/Elements/e/P20042>,
        <http://rdaregistry.info/Elements/e/P20043>,
        <http://rdaregistry.info/Elements/e/P20046>,
        <http://rdaregistry.info/Elements/e/P20047>,
        <http://rdaregistry.info/Elements/e/P20048>,
        <http://rdaregistry.info/Elements/e/P20049>,
        <http://rdaregistry.info/Elements/e/P20050>,
        <http://rdaregistry.info/Elements/e/P20051>,
        <http://rdaregistry.info/Elements/e/P20052>,
        <http://rdaregistry.info/Elements/e/P20054>,
        <http://rdaregistry.info/Elements/e/P20055>,
        <http://rdaregistry.info/Elements/e/P20056>,
        <http://rdaregistry.info/Elements/e/P20058>,
        <http://rdaregistry.info/Elements/e/P20257>,
        <http://rdaregistry.info/Elements/e/P20258>,
        <http://rdaregistry.info/Elements/e/P20276>,
        <http://rdaregistry.info/Elements/e/P20277>,
        <http://rdaregistry.info/Elements/e/P20279>,
        <http://rdaregistry.info/Elements/e/P20280>,
        <http://rdaregistry.info/Elements/e/P20283>,
        <http://rdaregistry.info/Elements/e/P20284>,
        <http://rdaregistry.info/Elements/e/P20287>,
        <http://rdaregistry.info/Elements/e/P20289>,
        <http://rdaregistry.info/Elements/e/P20292>,
        <http://rdaregistry.info/Elements/e/P20294>,
        <http://rdaregistry.info/Elements/e/P20295>,
        <http://rdaregistry.info/Elements/e/P20296>,
        <http://rdaregistry.info/Elements/e/object/P20053> ;
    reg:hasUnconstrained <http://rdaregistry.info/Elements/u/P60398> ;
    reg:lexicalAlias <http://rdaregistry.info/Elements/e/contributor.en> ;
    reg:name "contributor"@en ;
    reg:status <http://metadataregistry.org/uri/RegStatus/1001> ;
    rdfs:domain <http://rdaregistry.info/Elements/c/C10006> ;
    rdfs:isDefinedBy <http://rdaregistry.info/Elements/e/> ;
    rdfs:subPropertyOf <http://rdaregistry.info/Elements/e/P20301> ;
    skos:definition "Relates an expression to an agent contributing to an expression."@en ;
    skos:scopeNote "Contributors include editors, translators, arrangers of music, performers, etc."@en .

<http://metadataregistry.org/uri/RegStatus/1001> a skos:Concept ;
    skos:prefLabel "Published"@en .

<http://rdaregistry.info/Elements/e/> dc:title "RDA Expression properties"@en ;
    skos:note "Properties derived from RDA elements and relationship designators with the domain of RDA Expression."@en ;
    foaf:homepage <http://www.rdaregistry.info/Elements/e/> .

