@prefix dc: <http://purl.org/dc/elements/1.1/> .
@prefix foaf: <http://xmlns.com/foaf/0.1/> .
@prefix rdakit: <http://metadataregistry.org/uri/profile/rdakit/> .
@prefix rdf: <http://www.w3.org/1999/02/22-rdf-syntax-ns#> .
@prefix rdfs: <http://www.w3.org/2000/01/rdf-schema#> .
@prefix reg: <http://metadataregistry.org/uri/profile/regap/> .
@prefix skos: <http://www.w3.org/2004/02/skos/core#> .
@prefix xml: <http://www.w3.org/XML/1998/namespace> .
@prefix xsd: <http://www.w3.org/2001/XMLSchema#> .

<http://rdaregistry.info/Elements/w/P10002> a rdf:Property ;
    rdfs:label "has identifier for work"@en ;
    rdakit:instructionNumber "6.8" ;
    rdakit:toolkitDefinition "A character string uniquely associated with a work, or with a surrogate such as an authority record for a work."@en,
        "Una cadena de caracteres asociada con una obra, o un substituto de una obra (p.ej., un registro de autoridad)."@es,
        "Chaîne de caractères associée de manière unique à une œuvre ou à un substitut d’une œuvre (par exemple, une notice d’autorité)."@fr ;
    rdakit:toolkitLabel "identifier for work"@en,
        "identificador de la obra"@es,
        "identifiant de l’œuvre"@fr ;
    reg:hasUnconstrained <http://rdaregistry.info/Elements/u/P60052> ;
    reg:lexicalAlias <http://rdaregistry.info/Elements/w/identifierForWork.en> ;
    reg:name "identifierForWork"@en ;
    reg:status <http://metadataregistry.org/uri/RegStatus/1001> ;
    rdfs:domain <http://rdaregistry.info/Elements/c/C10001> ;
    rdfs:isDefinedBy <http://rdaregistry.info/Elements/w/> ;
    skos:definition "Relates a work to a character string uniquely associated with a work, or with a surrogate such as an authority record for a work."@en ;
    skos:scopeNote "The identifier serves to differentiate a work from other works."@en,
        "L’identifiant sert à distinguer cette œuvre d’autres œuvres."@fr .

<http://rdaregistry.info/Elements/w/P10003> a rdf:Property ;
    rdfs:label "has other distinguishing characteristic of work"@en,
        "har andra särskiljande egenskaper för verket"@sv ;
    rdakit:instructionNumber "6.6" ;
    rdakit:toolkitDefinition "A characteristic other than form of work, date of work, or place of origin of the work."@en,
        "Una característica distintiva de la forma de la obra, de la fecha de la obra o del lugar de origen de la obra."@es,
        "Caractéristique autre que la forme de l’œuvre, la date de l’œuvre ou le lieu d’origine de l’œuvre."@fr ;
    rdakit:toolkitLabel "other distinguishing characteristic of work"@en,
        "otra característica distintiva de la obra"@es,
        "autre caractéristique distinctive de l’œuvre"@fr,
        "andra särskiljande egenskaper för verket"@sv ;
    reg:hasUnconstrained <http://rdaregistry.info/Elements/u/P60054> ;
    reg:lexicalAlias <http://rdaregistry.info/Elements/w/otherDistinguishingCharacteristicOfWork.en> ;
    reg:name "otherDistinguishingCharacteristicOfWork"@en ;
    reg:status <http://metadataregistry.org/uri/RegStatus/1001> ;
    rdfs:domain <http://rdaregistry.info/Elements/c/C10001> ;
    rdfs:isDefinedBy <http://rdaregistry.info/Elements/w/> ;
    skos:definition "Relates a work to a characteristic other than form of work, date of work, or place of origin of the work."@en ;
    skos:scopeNote "The identifier serves to differentiate a work from another work with the same title or from the name of an agent."@en,
        "Elle sert à distinguer une œuvre d’une autre œuvre portant le même titre ou à la différencier du nom d’une personne, famille ou collectivité."@fr .

<http://rdaregistry.info/Elements/w/P10004> a rdf:Property ;
    rdfs:label "has form of work"@en,
        "har verkets form"@sv ;
    rdakit:instructionNumber "6.3" ;
    rdakit:toolkitDefinition "A class or genre to which a work belongs."@en,
        "Una clase o género al cual pertenece una obra."@es,
        "Catégorie ou genre auquel l’œuvre appartient."@fr ;
    rdakit:toolkitLabel "form of work"@en,
        "forma de la obra"@es,
        "forme de l’œuvre"@fr,
        "verkets form"@sv ;
    reg:hasUnconstrained <http://rdaregistry.info/Elements/u/P60058> ;
    reg:lexicalAlias <http://rdaregistry.info/Elements/w/formOfWork.en> ;
    reg:name "formOfWork"@en ;
    reg:status <http://metadataregistry.org/uri/RegStatus/1001> ;
    rdfs:domain <http://rdaregistry.info/Elements/c/C10001> ;
    rdfs:isDefinedBy <http://rdaregistry.info/Elements/w/> ;
    skos:definition "Relates a work to a class or genre to which a work belongs."@en .

<http://rdaregistry.info/Elements/w/P10012> a rdf:Property ;
    rdfs:label "has numbering of part"@en,
        "har numrering av del"@sv ;
    rdakit:instructionNumber "24.6" ;
    rdakit:toolkitDefinition "A designation of a sequencing of a part or parts within a larger work."@en,
        "Una designación de la secuencia de una parte o partes dentro de una obra mayor."@es,
        "Indication d’ordre séquentiel d’une ou de plusieurs parties à l’intérieur d’une œuvre plus vaste."@fr ;
    rdakit:toolkitLabel "numbering of part"@en,
        "numeración de la parte"@es,
        "numérotation d’une partie"@fr,
        "numrering av del"@sv ;
    reg:hasUnconstrained <http://rdaregistry.info/Elements/u/P60080> ;
    reg:lexicalAlias <http://rdaregistry.info/Elements/w/numberingOfPart.en> ;
    reg:name "numberingOfPart"@en ;
    reg:status <http://metadataregistry.org/uri/RegStatus/1001> ;
    rdfs:domain <http://rdaregistry.info/Elements/c/C10001> ;
    rdfs:isDefinedBy <http://rdaregistry.info/Elements/w/> ;
    skos:definition "Relates a work to a designation of a sequencing of a part or parts within a larger work."@en ;
    skos:scopeNote "Numbering includes a numeral, a letter, any other character, or the combination of these with or without an accompanying caption, and/or a chronological designation."@en .

<http://rdaregistry.info/Elements/w/P10072> a rdf:Property ;
    rdfs:label "has manifestation of work"@en,
        "har manifestation av verk"@sv ;
    rdakit:instructionNumber "17.7" ;
    rdakit:toolkitDefinition "A physical embodiment of a work."@en,
        "La materialización física de una expresión de una obra."@es,
        "Matérialisation d’une expression d’une œuvre."@fr ;
    rdakit:toolkitLabel "manifestation of work"@en,
        "manifestación de la obra"@es,
        "manifestation d’une œuvre"@fr,
        "manifestation av verk"@sv ;
    reg:hasSubproperty <http://rdaregistry.info/Elements/w/object/P10072> ;
    reg:lexicalAlias <http://rdaregistry.info/Elements/w/manifestationOfWork.en> ;
    reg:name "manifestationOfWork"@en ;
    reg:status <http://metadataregistry.org/uri/RegStatus/1001> ;
    rdfs:domain <http://rdaregistry.info/Elements/c/C10001> ;
    rdfs:isDefinedBy <http://rdaregistry.info/Elements/w/> ;
    skos:definition "Relates a work to a physical embodiment of a work."@en .

<http://rdaregistry.info/Elements/w/P10077> a rdf:Property ;
    rdfs:label "has academic degree"@en,
        "har akademisk grad"@sv ;
    rdakit:instructionNumber "7.9.2" ;
    rdakit:toolkitDefinition "A rank conferred as a guarantee of academic proficiency."@en,
        "Un rango conferido como garantía de capacidad acedémica."@es,
        "Grade conféré garantissant un niveau universitaire."@fr ;
    rdakit:toolkitLabel "academic degree"@en,
        "grado académico"@es,
        "diplôme universitaire"@fr,
        "akademisk grad"@sv ;
    reg:hasUnconstrained <http://rdaregistry.info/Elements/u/P60175> ;
    reg:lexicalAlias <http://rdaregistry.info/Elements/w/academicDegree.en> ;
    reg:name "academicDegree"@en ;
    reg:status <http://metadataregistry.org/uri/RegStatus/1001> ;
    rdfs:domain <http://rdaregistry.info/Elements/c/C10001> ;
    rdfs:isDefinedBy <http://rdaregistry.info/Elements/w/> ;
    skos:definition "Relates a work to a rank conferred as a guarantee of academic proficiency."@en .

<http://rdaregistry.info/Elements/w/P10078> a rdf:Property ;
    rdfs:label "has expression of work"@en,
        "har uttryck för verk"@sv ;
    rdakit:instructionNumber "17.5" ;
    rdakit:toolkitDefinition "A realization of a work in the form of alpha-numeric, musical or choreographic notation, sound, image, object, movement, etc., or any combination of such forms."@en,
        "Una realización de la obra en la forma de notaciones alfanumérica, musical o coreográfica, sonido, imagen, movimiento, etc. o en cualquier combinación de tales formas."@es,
        "Réalisation d’une œuvre sous la forme d’une notation alphanumérique, musicale ou chorégraphique, de son, d’image, d’objet, de mouvement, etc. ou de toute combinaison de ces formes."@fr ;
    rdakit:toolkitLabel "expression of work"@en,
        "expresión de la obra"@es,
        "expression d’une œuvre"@fr,
        "uttryck för verk"@sv ;
    reg:hasSubproperty <http://rdaregistry.info/Elements/w/object/P10078> ;
    reg:lexicalAlias <http://rdaregistry.info/Elements/w/expressionOfWork.en> ;
    reg:name "expressionOfWork"@en ;
    reg:status <http://metadataregistry.org/uri/RegStatus/1001> ;
    rdfs:domain <http://rdaregistry.info/Elements/c/C10001> ;
    rdfs:isDefinedBy <http://rdaregistry.info/Elements/w/> ;
    skos:definition "Relates a work to a realization of a work in the form of alpha-numeric, musical or choreographic notation, sound, image, object, movement, etc., or any combination of such forms."@en .

<http://rdaregistry.info/Elements/w/P10079> a rdf:Property ;
    rdfs:label "has numeric designation of musical work"@en ;
    rdakit:instructionNumber "6.16" ;
    rdakit:toolkitDefinition "A serial number, opus number, or thematic index number assigned to a musical work by a composer, publisher, or a musicologist."@en,
        "Un número seriado, número de opus o número de índice temático, asignado a una obra musical por el compositor, el editor o un musicólogo."@es,
        "Numéro d’ordre, numéro d’opus ou numéro de catalogue thématique attribué à une œuvre musicale par un compositeur, un éditeur ou un musicologue."@fr ;
    rdakit:toolkitLabel "numeric designation of musical work"@en,
        "designación numérica de una obra musical"@es,
        "référence numérique d’une œuvre musicale"@fr ;
    reg:hasUnconstrained <http://rdaregistry.info/Elements/u/P60315> ;
    reg:lexicalAlias <http://rdaregistry.info/Elements/w/numericDesignationOfMusicalWork.en> ;
    reg:name "numericDesignationOfMusicalWork"@en ;
    reg:status <http://metadataregistry.org/uri/RegStatus/1001> ;
    rdfs:domain <http://rdaregistry.info/Elements/c/C10001> ;
    rdfs:isDefinedBy <http://rdaregistry.info/Elements/w/> ;
    skos:definition "Relates a work to a serial number, opus number, or thematic index number assigned to a musical work by a composer, publisher, or a musicologist."@en ;
    skos:scopeNote "A numeric designation of a musical work includes a caption such as e.g., no., op., BWV, and it may include a numeral, a letter, a word, any other character, or the combination of these."@en .

<http://rdaregistry.info/Elements/w/P10084> a rdf:Property ;
    rdfs:label "has system of organization"@en,
        "har arkivstruktur"@sv ;
    rdakit:instructionNumber "7.8" ;
    rdakit:toolkitDefinition "A system of arranging materials in an archival resource or a collection."@en,
        "Un sistema de arreglo de los materiales dentro de un recurso de archivo o de una colección."@es,
        "Système de classement des éléments matériels d’une ressource archivistique ou d’une collection."@fr ;
    rdakit:toolkitLabel "system of organization"@en,
        "sistema de organización"@es,
        "système d’organisation"@fr,
        "arkivstruktur"@sv ;
    reg:hasUnconstrained <http://rdaregistry.info/Elements/u/P60348> ;
    reg:lexicalAlias <http://rdaregistry.info/Elements/w/systemOfOrganization.en> ;
    reg:name "systemOfOrganization"@en ;
    reg:status <http://metadataregistry.org/uri/RegStatus/1001> ;
    rdfs:domain <http://rdaregistry.info/Elements/c/C10001> ;
    rdfs:isDefinedBy <http://rdaregistry.info/Elements/w/> ;
    skos:definition "Relates a work to a system of arranging materials in an archival resource or a collection."@en .

<http://rdaregistry.info/Elements/w/P10199> a rdf:Property ;
    rdfs:label "has epoch"@en,
        "har epok"@sv ;
    rdakit:instructionNumber "7.6" ;
    rdakit:toolkitDefinition "An arbitrary moment in time to which measurements of position for a body or orientation for an orbit are referred."@en,
        "Un momento arbitrario en el tiempo al cual hacen referencia las medidas de posición de un cuerpo o de orientación de una órbita."@es,
        "Moment arbitraire dans le temps auquel les mesures de position pour un corps céleste ou l’orientation pour une orbite font référence."@fr ;
    rdakit:toolkitLabel "epoch"@en,
        "época"@es,
        "époque"@fr,
        "epok"@sv ;
    reg:hasUnconstrained <http://rdaregistry.info/Elements/u/P60472> ;
    reg:lexicalAlias <http://rdaregistry.info/Elements/w/epoch.en> ;
    reg:name "epoch"@en ;
    reg:status <http://metadataregistry.org/uri/RegStatus/1001> ;
    rdfs:domain <http://rdaregistry.info/Elements/c/C10001> ;
    rdfs:isDefinedBy <http://rdaregistry.info/Elements/w/> ;
    skos:definition "Relates a work to an arbitrary moment in time to which measurements of position for a body or orientation for an orbit are referred."@en .

<http://rdaregistry.info/Elements/w/P10208> a rdf:Property ;
    rdfs:label "has granting institution or faculty"@en ;
    rdakit:instructionNumber "7.9.3" ;
    rdakit:toolkitDefinition "An institution or faculty conferring an academic degree on a candidate."@en,
        "Una institución o facultad que confiere un grado académico a un candidato."@es,
        "Institution ou faculté conférant un diplôme universitaire à un candidat."@fr ;
    rdakit:toolkitLabel "granting institution or faculty"@en,
        "institución o facultad otorgante"@es,
        "institution ou faculté habilitée à conférer un diplôme universitaire"@fr ;
    reg:hasUnconstrained <http://rdaregistry.info/Elements/u/P60483> ;
    reg:lexicalAlias <http://rdaregistry.info/Elements/w/grantingInstitutionOrFaculty.en> ;
    reg:name "grantingInstitutionOrFaculty"@en ;
    reg:status <http://metadataregistry.org/uri/RegStatus/1001> ;
    rdfs:domain <http://rdaregistry.info/Elements/c/C10001> ;
    rdfs:isDefinedBy <http://rdaregistry.info/Elements/w/> ;
    skos:definition "Relates a work to an institution or faculty conferring an academic degree on a candidate."@en .

<http://rdaregistry.info/Elements/w/P10209> a rdf:Property ;
    rdfs:label "has dissertation or thesis information"@en,
        "har uppgifter om akademisk avhandling och dylikt"@sv ;
    rdakit:instructionNumber "7.9" ;
    rdakit:toolkitDefinition "A statement identifying an academic institution, degree, and year for which a work was presented."@en,
        "Información relativa a una obra presentada como parte de los requisitos formales de un grado académico."@es,
        "Information relative à une œuvre présentée comme faisant partie des conditions formelles requises pour l’obtention d’un diplôme universitaire."@fr ;
    rdakit:toolkitLabel "dissertation or thesis information"@en,
        "información de una disertación o tesis"@es,
        "information sur la thèse ou le mémoire"@fr,
        "uppgifter om akademisk avhandling och dylikt"@sv ;
    reg:hasUnconstrained <http://rdaregistry.info/Elements/u/P60489> ;
    reg:lexicalAlias <http://rdaregistry.info/Elements/w/dissertationOrThesisInformation.en> ;
    reg:name "dissertationOrThesisInformation"@en ;
    reg:status <http://metadataregistry.org/uri/RegStatus/1001> ;
    rdfs:domain <http://rdaregistry.info/Elements/c/C10001> ;
    rdfs:isDefinedBy <http://rdaregistry.info/Elements/w/> ;
    skos:definition "Relates a work to a statement identifying an academic institution, degree, and year for which a work was presented."@en .

<http://rdaregistry.info/Elements/w/P10210> a rdf:Property ;
    rdfs:label "has history of work"@en,
        "har verkets historia"@sv ;
    rdakit:instructionNumber "6.7" ;
    rdakit:toolkitDefinition "A summary of information about the history of a work."@en,
        "Información relativa a la historia de una obra."@es,
        "Information sur l’histoire d’une œuvre."@fr ;
    rdakit:toolkitLabel "history of work"@en,
        "historia de la obra"@es,
        "historique de l’œuvre"@fr,
        "verkets historia"@sv ;
    reg:hasUnconstrained <http://rdaregistry.info/Elements/u/P60491> ;
    reg:lexicalAlias <http://rdaregistry.info/Elements/w/historyOfWork.en> ;
    reg:name "historyOfWork"@en ;
    reg:status <http://metadataregistry.org/uri/RegStatus/1001> ;
    rdfs:domain <http://rdaregistry.info/Elements/c/C10001> ;
    rdfs:isDefinedBy <http://rdaregistry.info/Elements/w/> ;
    skos:definition "Relates a work to a summary of information about the history of a work."@en .

<http://rdaregistry.info/Elements/w/P10214> a rdf:Property ;
    rdfs:label "has equinox"@en,
        "har ekvinoktium"@sv ;
    rdakit:instructionNumber "7.5" ;
    rdakit:toolkitDefinition "A point of intersection of the ecliptic and the celestial equator, occupied by the sun when its declination is 0°."@en,
        "Uno de los dos puntos de intersección de la eclíptica y el Ecuador celeste, ocupada por el sol cuando su declinación es 0°."@es,
        "L’un des deux points d’intersection de l’écliptique et de l’équateur céleste, occupé par le soleil quand sa déclinaison est de 0°."@fr ;
    rdakit:toolkitLabel "equinox"@en,
        "equinoccio"@es,
        "équinoxe"@fr,
        "ekvinoktium"@sv ;
    reg:hasUnconstrained <http://rdaregistry.info/Elements/u/P60506> ;
    reg:lexicalAlias <http://rdaregistry.info/Elements/w/equinox.en> ;
    reg:name "equinox"@en ;
    reg:status <http://metadataregistry.org/uri/RegStatus/1001> ;
    rdfs:domain <http://rdaregistry.info/Elements/c/C10001> ;
    rdfs:isDefinedBy <http://rdaregistry.info/Elements/w/> ;
    skos:definition "Relates a work to a point of intersection of the ecliptic and the celestial equator, occupied by the sun when its declination is 0°."@en .

<http://rdaregistry.info/Elements/w/P10215> a rdf:Property ;
    rdfs:label "has year degree granted"@en,
        "har år när examen avlades"@sv ;
    rdakit:instructionNumber "7.9.4" ;
    rdakit:toolkitDefinition "A calendar year in which a granting institution or faculty conferred an academic degree on a candidate."@en,
        "El año calendario en el que una institución o cuerpo docente otorgante confiere un grado académico a un candidato."@es,
        "L’année civile de remise de diplôme à un candidat par une institution ou une faculté habilitée à conférer un diplôme universitaire."@fr ;
    rdakit:toolkitLabel "year degree granted"@en,
        "año de otorgación del grado"@es,
        "année d’obtention d’un diplôme universitaire"@fr,
        "år när examen avlades"@sv ;
    reg:hasUnconstrained <http://rdaregistry.info/Elements/u/P60514> ;
    reg:lexicalAlias <http://rdaregistry.info/Elements/w/yearDegreeGranted.en> ;
    reg:name "yearDegreeGranted"@en ;
    reg:status <http://metadataregistry.org/uri/RegStatus/1001> ;
    rdfs:domain <http://rdaregistry.info/Elements/c/C10001> ;
    rdfs:isDefinedBy <http://rdaregistry.info/Elements/w/> ;
    skos:definition "Relates a work to a calendar year in which a granting institution or faculty conferred an academic degree on a candidate."@en .

<http://rdaregistry.info/Elements/w/P10216> a rdf:Property ;
    rdfs:label "has coverage of content"@en,
        "har innehållets täckning"@sv ;
    rdakit:instructionNumber "7.3" ;
    rdakit:toolkitDefinition "A chronological or geographic coverage of the content of a work."@en,
        "La cobertura cronológica o geográfica del contenido de un recurso."@es,
        "La couverture chronologique ou géographique du contenu d’une ressource."@fr ;
    rdakit:toolkitLabel "coverage of content"@en,
        "cobertura del contenido"@es,
        "couverture du contenu"@fr,
        "innehållets täckning"@sv ;
    reg:hasUnconstrained <http://rdaregistry.info/Elements/u/P60518> ;
    reg:lexicalAlias <http://rdaregistry.info/Elements/w/coverageOfContent.en> ;
    reg:name "coverageOfContent"@en ;
    reg:status <http://metadataregistry.org/uri/RegStatus/1001> ;
    rdfs:domain <http://rdaregistry.info/Elements/c/C10001> ;
    rdfs:isDefinedBy <http://rdaregistry.info/Elements/w/> ;
    skos:definition "Relates a work to a chronological or geographic coverage of the content of a work."@en .

<http://rdaregistry.info/Elements/w/P10217> a rdf:Property ;
    rdfs:label "has intended audience"@en,
        "har målgrupp"@sv ;
    rdakit:instructionNumber "7.7" ;
    rdakit:toolkitDefinition "A category of user for which the content of a work is intended, or for whom the content is considered suitable."@en,
        "La clase de usuario a la cual va dirigido el contenido de un recurso, o para quienes el contenido se considera apropiado."@es,
        "La classe d’utilisateurs à laquelle est destiné, ou supposé convenir, le contenu d’une ressource."@fr ;
    rdakit:toolkitLabel "intended audience"@en,
        "audiencia prevista"@es,
        "public cible"@fr,
        "målgrupp"@sv ;
    reg:hasUnconstrained <http://rdaregistry.info/Elements/u/P60520> ;
    reg:lexicalAlias <http://rdaregistry.info/Elements/w/intendedAudience.en> ;
    reg:name "intendedAudience"@en ;
    reg:status <http://metadataregistry.org/uri/RegStatus/1001> ;
    rdfs:domain <http://rdaregistry.info/Elements/c/C10001> ;
    rdfs:isDefinedBy <http://rdaregistry.info/Elements/w/> ;
    skos:definition "Relates a work to a category of user for which the content of a work is intended, or for whom the content is considered suitable."@en ;
    skos:scopeNote "La classe d’utilisateurs est définie soit par tranche d’âge (par exemple, enfants, jeunes adultes, adultes), soit par niveau d’éducation (par exemple, primaire, secondaire), soit par type de handicap ou par toute autre catégorisation."@fr .

<http://rdaregistry.info/Elements/w/P10218> a rdf:Property ;
    rdfs:label "has place of origin of work"@en,
        "har ursprungsort för verket"@sv ;
    rdakit:instructionNumber "6.5" ;
    rdakit:toolkitDefinition "A country or other territorial jurisdiction from which a work originated."@en,
        "El país u otra jurisdicción territorial en la cual se originó la obra."@es,
        "Le pays ou tout territoire d’où l’œuvre est originaire."@fr ;
    rdakit:toolkitLabel "place of origin of work"@en,
        "lugar de origen de la obra"@es,
        "lieu d’origine de l’œuvre"@fr,
        "ursprungsort för verket"@sv ;
    reg:hasUnconstrained <http://rdaregistry.info/Elements/u/P60523> ;
    reg:lexicalAlias <http://rdaregistry.info/Elements/w/placeOfOriginOfWork.en> ;
    reg:name "placeOfOriginOfWork"@en ;
    reg:status <http://metadataregistry.org/uri/RegStatus/1001> ;
    rdfs:domain <http://rdaregistry.info/Elements/c/C10001> ;
    rdfs:isDefinedBy <http://rdaregistry.info/Elements/w/> ;
    skos:definition "Relates a work to a country or other territorial jurisdiction from which a work originated."@en .

<http://rdaregistry.info/Elements/w/P10219> a rdf:Property ;
    rdfs:label "has date of work"@en,
        "har tid för verket"@sv ;
    rdakit:instructionNumber "6.4" ;
    rdakit:toolkitDefinition "An earliest date associated with a work."@en,
        "La fecha más antigua asociada con una obra."@es,
        "La date la plus ancienne associée à une œuvre."@fr ;
    rdakit:toolkitLabel "date of work"@en,
        "fecha de la obra"@es,
        "date de l’œuvre"@fr,
        "tid för verket"@sv ;
    reg:hasUnconstrained <http://rdaregistry.info/Elements/u/P60527> ;
    reg:lexicalAlias <http://rdaregistry.info/Elements/w/dateOfWork.en> ;
    reg:name "dateOfWork"@en ;
    reg:status <http://metadataregistry.org/uri/RegStatus/1001> ;
    rdfs:domain <http://rdaregistry.info/Elements/c/C10001> ;
    rdfs:isDefinedBy <http://rdaregistry.info/Elements/w/> ;
    skos:definition "Relates a work to an earliest date associated with a work."@en .

<http://rdaregistry.info/Elements/w/P10220> a rdf:Property ;
    rdfs:label "has medium of performance"@en ;
    rdakit:instructionNumber "6.15" ;
    rdakit:toolkitDefinition "An instrument, voice, and/or ensemble for which a musical work was originally conceived."@en,
        "El instrumento, instrumentos, voz, voces, etc., para los cuales fue originalmente concebida una obra musical."@es,
        "Le ou les instruments, la ou les voix, etc. auxquels une œuvre musicale est originellement destinée."@fr ;
    rdakit:toolkitLabel "medium of performance"@en,
        "medio de interpretación"@es,
        "distribution d’exécution"@fr ;
    reg:hasUnconstrained <http://rdaregistry.info/Elements/u/P60536> ;
    reg:lexicalAlias <http://rdaregistry.info/Elements/w/mediumOfPerformance.en> ;
    reg:name "mediumOfPerformance"@en ;
    reg:status <http://metadataregistry.org/uri/RegStatus/1001> ;
    rdfs:domain <http://rdaregistry.info/Elements/c/C10001> ;
    rdfs:isDefinedBy <http://rdaregistry.info/Elements/w/> ;
    skos:definition "Relates a work to an instrument, voice, or ensemble for which a musical work was originally conceived."@en .

<http://rdaregistry.info/Elements/w/P10221> a rdf:Property ;
    rdfs:label "has key"@en,
        "har tonart"@sv ;
    rdakit:instructionNumber "6.17" ;
    rdakit:toolkitDefinition "A set of pitch relationships that establishes the tonal centre, or principal tonal centre, of a musical work."@en,
        "El conjunto de relaciones tonales que establece el centro tonal, o el centro tonal principal, de una obra musical."@es,
        "L’ensemble des rapports entre les hauteurs de sons qui détermine le centre tonal ou le principal centre tonal d’une œuvre musicale."@fr ;
    rdakit:toolkitLabel "key"@en,
        "tonalidad"@es,
        "tonalité"@fr,
        "tonart"@sv ;
    reg:hasUnconstrained <http://rdaregistry.info/Elements/u/P60580> ;
    reg:lexicalAlias <http://rdaregistry.info/Elements/w/key.en> ;
    reg:name "key"@en ;
    reg:status <http://metadataregistry.org/uri/RegStatus/1001> ;
    rdfs:domain <http://rdaregistry.info/Elements/c/C10001> ;
    rdfs:isDefinedBy <http://rdaregistry.info/Elements/w/> ;
    skos:definition "Relates a work to a set of pitch relationships that establishes a tonal centre, or principal tonal centre, of a musical work."@en ;
    skos:scopeNote "Key is indicated by its pitch name and its mode, when it is major or minor."@en .

<http://rdaregistry.info/Elements/w/P10222> a rdf:Property ;
    rdfs:label "has nature of content"@en,
        "har innehållets karaktär"@sv ;
    rdakit:instructionNumber "7.2" ;
    rdakit:toolkitDefinition "A specific character of the primary content of a work."@en,
        "El carácter específico del contenido primario del recurso (p.ej., artículos jurídicos; informe provisional)."@es,
        "La caractéristique spécifique du contenu principal d’une ressource (par exemple, articles juridiques, rapport d’étape)."@fr ;
    rdakit:toolkitLabel "nature of content"@en,
        "naturaleza del contenido"@es,
        "nature du contenu"@fr,
        "innehållets karaktär"@sv ;
    reg:hasUnconstrained <http://rdaregistry.info/Elements/u/P60584> ;
    reg:lexicalAlias <http://rdaregistry.info/Elements/w/natureOfContent.en> ;
    reg:name "natureOfContent"@en ;
    reg:status <http://metadataregistry.org/uri/RegStatus/1001> ;
    rdfs:domain <http://rdaregistry.info/Elements/c/C10001> ;
    rdfs:isDefinedBy <http://rdaregistry.info/Elements/w/> ;
    skos:definition "Relates a work to a specific character of the primary content of a work."@en .

<http://rdaregistry.info/Elements/w/P10230> a rdf:Property ;
    reg:hasSubproperty <http://rdaregistry.info/Elements/w/P10100>,
        <http://rdaregistry.info/Elements/w/P10118> ;
    reg:status <http://metadataregistry.org/uri/RegStatus/1008> ;
    rdfs:isDefinedBy <http://rdaregistry.info/Elements/w/> .

<http://rdaregistry.info/Elements/w/P10239> a rdf:Property ;
    rdfs:label "is video music (work)"@en ;
    rdakit:instructionNumber "24.5" ;
    rdakit:toolkitDefinition "A musical work that is used in a video."@en,
        "Una obra musical utilizada en un video."@es,
        "Œuvre musicale utilisée dans une vidéo."@fr ;
    rdakit:toolkitLabel "video music (work)"@en,
        "música de video (obra)"@es,
        "musique de vidéo (œuvre)"@fr ;
    reg:hasSubproperty <http://rdaregistry.info/Elements/w/object/P10239> ;
    reg:hasUnconstrained <http://rdaregistry.info/Elements/u/P60725> ;
    reg:lexicalAlias <http://rdaregistry.info/Elements/w/videoMusicWork.en> ;
    reg:name "videoMusicWork"@en ;
    reg:status <http://metadataregistry.org/uri/RegStatus/1001> ;
    rdfs:domain <http://rdaregistry.info/Elements/c/C10001> ;
    rdfs:isDefinedBy <http://rdaregistry.info/Elements/w/> ;
    rdfs:subPropertyOf <http://rdaregistry.info/Elements/w/P10237> ;
    skos:definition "Relates a work to a musical work that is used in a video."@en .

<http://rdaregistry.info/Elements/w/P10240> a rdf:Property ;
    rdfs:label "is music for video (work)"@en ;
    rdakit:instructionNumber "24.5" ;
    rdakit:toolkitDefinition "A work that uses a musical work in a video."@en,
        "Una obra que utiliza la obra musical en un video."@es,
        "Œuvre qui utilise l’œuvre musicale dans une vidéo."@fr ;
    rdakit:toolkitLabel "music for video (work)"@en,
        "música para video (obra)"@es,
        "musique pour la vidéo (œuvre)"@fr ;
    reg:hasSubproperty <http://rdaregistry.info/Elements/w/object/P10240> ;
    reg:hasUnconstrained <http://rdaregistry.info/Elements/u/P60726> ;
    reg:lexicalAlias <http://rdaregistry.info/Elements/w/musicForVideoWork.en> ;
    reg:name "musicForVideoWork"@en ;
    reg:status <http://metadataregistry.org/uri/RegStatus/1001> ;
    rdfs:domain <http://rdaregistry.info/Elements/c/C10001> ;
    rdfs:isDefinedBy <http://rdaregistry.info/Elements/w/> ;
    rdfs:subPropertyOf <http://rdaregistry.info/Elements/w/P10238> ;
    skos:definition "Relates a work to a work that uses a musical work in a video."@en .

<http://rdaregistry.info/Elements/w/P10241> a rdf:Property ;
    rdfs:label "is television program music (work)"@en ;
    rdakit:instructionNumber "24.5" ;
    rdakit:toolkitDefinition "A musical work that is used in a television program."@en,
        "Una obra musical utilizada en un programa de televisión."@es,
        "Œuvre musicale utilisée dans une émission de télévision."@fr ;
    rdakit:toolkitLabel "television program music (work)"@en,
        "música de programa de televisión (obra)"@es,
        "musique d’émission de télévision (œuvre)"@fr ;
    reg:hasSubproperty <http://rdaregistry.info/Elements/w/object/P10241> ;
    reg:hasUnconstrained <http://rdaregistry.info/Elements/u/P60727> ;
    reg:lexicalAlias <http://rdaregistry.info/Elements/w/televisionProgramMusicWork.en> ;
    reg:name "televisionProgramMusicWork"@en ;
    reg:status <http://metadataregistry.org/uri/RegStatus/1001> ;
    rdfs:domain <http://rdaregistry.info/Elements/c/C10001> ;
    rdfs:isDefinedBy <http://rdaregistry.info/Elements/w/> ;
    rdfs:subPropertyOf <http://rdaregistry.info/Elements/w/P10237> ;
    skos:definition "Relates a work to a musical work that is used in a television program."@en .

<http://rdaregistry.info/Elements/w/P10242> a rdf:Property ;
    rdfs:label "is music for television program (work)"@en ;
    rdakit:instructionNumber "24.5" ;
    rdakit:toolkitDefinition "A work that uses a musical work in a television program."@en,
        "Una obra que utliza la obra musical en un programa de televisión."@es,
        "Œuvre qui utilise l’œuvre musicale dans une émission de télévision."@fr ;
    rdakit:toolkitLabel "music for television program (work)"@en,
        "música para programa de televisión (obra)"@es,
        "musique pour l’émission de télévision (œuvre)"@fr ;
    reg:hasSubproperty <http://rdaregistry.info/Elements/w/object/P10242> ;
    reg:hasUnconstrained <http://rdaregistry.info/Elements/u/P60728> ;
    reg:lexicalAlias <http://rdaregistry.info/Elements/w/musicForTelevisionProgramWork.en> ;
    reg:name "musicForTelevisionProgramWork"@en ;
    reg:status <http://metadataregistry.org/uri/RegStatus/1001> ;
    rdfs:domain <http://rdaregistry.info/Elements/c/C10001> ;
    rdfs:isDefinedBy <http://rdaregistry.info/Elements/w/> ;
    rdfs:subPropertyOf <http://rdaregistry.info/Elements/w/P10238> ;
    skos:definition "Relates a work to a work that uses a musical work in a television program."@en .

<http://rdaregistry.info/Elements/w/P10243> a rdf:Property ;
    rdfs:label "is radio program music (work)"@en ;
    rdakit:instructionNumber "24.5" ;
    rdakit:toolkitDefinition "A musical work that is used in a radio program."@en,
        "Una obra musical utilizada en un programa de radio."@es,
        "Œuvre musicale utilisée dans une émission de radio."@fr ;
    rdakit:toolkitLabel "radio program music (work)"@en,
        "música de programa radial (obra)"@es,
        "musique d’émission de radio (œuvre)"@fr ;
    reg:hasSubproperty <http://rdaregistry.info/Elements/w/object/P10243> ;
    reg:hasUnconstrained <http://rdaregistry.info/Elements/u/P60729> ;
    reg:lexicalAlias <http://rdaregistry.info/Elements/w/radioProgramMusicWork.en> ;
    reg:name "radioProgramMusicWork"@en ;
    reg:status <http://metadataregistry.org/uri/RegStatus/1001> ;
    rdfs:domain <http://rdaregistry.info/Elements/c/C10001> ;
    rdfs:isDefinedBy <http://rdaregistry.info/Elements/w/> ;
    rdfs:subPropertyOf <http://rdaregistry.info/Elements/w/P10237> ;
    skos:definition "Relates a work to a musical work that is used in a radio program."@en .

<http://rdaregistry.info/Elements/w/P10244> a rdf:Property ;
    rdfs:label "is music for radio program (work)"@en ;
    rdakit:instructionNumber "24.5" ;
    rdakit:toolkitDefinition "A work that uses a musical work in a radio program."@en,
        "Una obra que utiliza la obra musical en un programa de radio."@es,
        "Œuvre qui utilise l’œuvre musicale dans une émission de radio."@fr ;
    rdakit:toolkitLabel "music for radio program (work)"@en,
        "música para programa radial (obra)"@es,
        "musique pour l’émission de radio (œuvre)"@fr ;
    reg:hasSubproperty <http://rdaregistry.info/Elements/w/object/P10244> ;
    reg:hasUnconstrained <http://rdaregistry.info/Elements/u/P60730> ;
    reg:lexicalAlias <http://rdaregistry.info/Elements/w/musicForRadioProgramWork.en> ;
    reg:name "musicForRadioProgramWork"@en ;
    reg:status <http://metadataregistry.org/uri/RegStatus/1001> ;
    rdfs:domain <http://rdaregistry.info/Elements/c/C10001> ;
    rdfs:isDefinedBy <http://rdaregistry.info/Elements/w/> ;
    rdfs:subPropertyOf <http://rdaregistry.info/Elements/w/P10238> ;
    skos:definition "Relates a work to a work that uses a musical work in a radio program."@en .

<http://rdaregistry.info/Elements/w/P10245> a rdf:Property ;
    rdfs:label "is music for motion picture (work)"@en ;
    rdakit:instructionNumber "24.5" ;
    rdakit:toolkitDefinition "A work that uses a musical work in a motion picture."@en,
        "Una obra que utiliza la obra musical en una película."@es,
        "Œuvre qui utilise l’œuvre musicale dans un film."@fr ;
    rdakit:toolkitLabel "music for motion picture (work)"@en,
        "musica para película cinematográfica (obra)"@es,
        "musique pour le film (œuvre)"@fr ;
    reg:hasSubproperty <http://rdaregistry.info/Elements/w/object/P10245> ;
    reg:hasUnconstrained <http://rdaregistry.info/Elements/u/P60731> ;
    reg:lexicalAlias <http://rdaregistry.info/Elements/w/musicForMotionPictureWork.en> ;
    reg:name "musicForMotionPictureWork"@en ;
    reg:status <http://metadataregistry.org/uri/RegStatus/1001> ;
    rdfs:domain <http://rdaregistry.info/Elements/c/C10001> ;
    rdfs:isDefinedBy <http://rdaregistry.info/Elements/w/> ;
    rdfs:subPropertyOf <http://rdaregistry.info/Elements/w/P10238> ;
    skos:definition "Relates a work to a work that uses a musical work in a motion picture."@en .

<http://rdaregistry.info/Elements/w/P10246> a rdf:Property ;
    rdfs:label "is motion picture music (work)"@en ;
    rdakit:instructionNumber "24.5" ;
    rdakit:toolkitDefinition "A musical work that is used in a motion picture."@en,
        "Una obra musical que es utlizada en una película cinematográfica"@es,
        "Œuvre musicale utilisée dans un film."@fr ;
    rdakit:toolkitLabel "motion picture music (work)"@en,
        "música de película cinematográfica"@es,
        "musique de film (œuvre)"@fr ;
    reg:hasSubproperty <http://rdaregistry.info/Elements/w/object/P10246> ;
    reg:hasUnconstrained <http://rdaregistry.info/Elements/u/P60732> ;
    reg:lexicalAlias <http://rdaregistry.info/Elements/w/motionPictureMusicWork.en> ;
    reg:name "motionPictureMusicWork"@en ;
    reg:status <http://metadataregistry.org/uri/RegStatus/1001> ;
    rdfs:domain <http://rdaregistry.info/Elements/c/C10001> ;
    rdfs:isDefinedBy <http://rdaregistry.info/Elements/w/> ;
    rdfs:subPropertyOf <http://rdaregistry.info/Elements/w/P10237> ;
    skos:definition "Relates a work to a musical work that is used in a motion picture."@en .

<http://rdaregistry.info/Elements/w/P10308> a rdf:Property ;
    rdfs:label "has related expression (work)"@en ;
    reg:hasSubproperty <http://rdaregistry.info/Elements/w/datatype/P10308>,
        <http://rdaregistry.info/Elements/w/object/P10308> ;
    reg:hasUnconstrained <http://rdaregistry.info/Elements/u/P60313> ;
    reg:lexicalAlias <http://rdaregistry.info/Elements/w/relatedExpressionWork.en> ;
    reg:name "relatedExpressionWork"@en ;
    reg:status <http://metadataregistry.org/uri/RegStatus/1001> ;
    rdfs:domain <http://rdaregistry.info/Elements/c/C10001> ;
    rdfs:isDefinedBy <http://rdaregistry.info/Elements/w/> ;
    rdfs:subPropertyOf <http://rdaregistry.info/Elements/w/P10307> ;
    skos:definition "Relates a work to an expression associated with a work being described."@en .

<http://rdaregistry.info/Elements/w/P10309> a rdf:Property ;
    rdfs:label "has related manifestation (work)"@en ;
    reg:hasSubproperty <http://rdaregistry.info/Elements/w/datatype/P10309>,
        <http://rdaregistry.info/Elements/w/object/P10309> ;
    reg:hasUnconstrained <http://rdaregistry.info/Elements/u/P60313> ;
    reg:lexicalAlias <http://rdaregistry.info/Elements/w/relatedManifestationWork.en> ;
    reg:name "relatedManifestationWork"@en ;
    reg:status <http://metadataregistry.org/uri/RegStatus/1001> ;
    rdfs:domain <http://rdaregistry.info/Elements/c/C10001> ;
    rdfs:isDefinedBy <http://rdaregistry.info/Elements/w/> ;
    rdfs:subPropertyOf <http://rdaregistry.info/Elements/w/P10307> ;
    skos:definition "Relates a work to a manifestation associated with a work being described."@en .

<http://rdaregistry.info/Elements/w/P10310> a rdf:Property ;
    rdfs:label "has related item (work)"@en ;
    reg:hasSubproperty <http://rdaregistry.info/Elements/w/datatype/P10310>,
        <http://rdaregistry.info/Elements/w/object/P10310> ;
    reg:hasUnconstrained <http://rdaregistry.info/Elements/u/P60313> ;
    reg:lexicalAlias <http://rdaregistry.info/Elements/w/relatedItemWork.en> ;
    reg:name "relatedItemWork"@en ;
    reg:status <http://metadataregistry.org/uri/RegStatus/1001> ;
    rdfs:domain <http://rdaregistry.info/Elements/c/C10001> ;
    rdfs:isDefinedBy <http://rdaregistry.info/Elements/w/> ;
    rdfs:subPropertyOf <http://rdaregistry.info/Elements/w/P10307> ;
    skos:definition "Relates a work to an item associated with a work being described."@en .

<http://rdaregistry.info/Elements/w/P10312> a rdf:Property ;
    rdfs:label "has related person (work)"@en ;
    reg:hasSubproperty <http://rdaregistry.info/Elements/w/datatype/P10312>,
        <http://rdaregistry.info/Elements/w/object/P10312> ;
    reg:lexicalAlias <http://rdaregistry.info/Elements/w/relatedPersonWork.en> ;
    reg:name "relatedPersonWork"@en ;
    reg:status <http://metadataregistry.org/uri/RegStatus/1001> ;
    rdfs:domain <http://rdaregistry.info/Elements/c/C10001> ;
    rdfs:isDefinedBy <http://rdaregistry.info/Elements/w/> ;
    rdfs:subPropertyOf <http://rdaregistry.info/Elements/w/P10311> ;
    skos:definition "Relates a work to a person associated with a work being described."@en .

<http://rdaregistry.info/Elements/w/P10313> a rdf:Property ;
    rdfs:label "has related family (work)"@en ;
    reg:hasSubproperty <http://rdaregistry.info/Elements/w/datatype/P10313>,
        <http://rdaregistry.info/Elements/w/object/P10313> ;
    reg:lexicalAlias <http://rdaregistry.info/Elements/w/relatedFamilyWork.en> ;
    reg:name "relatedFamilyWork"@en ;
    reg:status <http://metadataregistry.org/uri/RegStatus/1001> ;
    rdfs:domain <http://rdaregistry.info/Elements/c/C10001> ;
    rdfs:isDefinedBy <http://rdaregistry.info/Elements/w/> ;
    rdfs:subPropertyOf <http://rdaregistry.info/Elements/w/P10315> ;
    skos:definition "Relates a work to a family associated with a work being described."@en .

<http://rdaregistry.info/Elements/w/P10314> a rdf:Property ;
    rdfs:label "has related corporate body (work)"@en ;
    reg:hasSubproperty <http://rdaregistry.info/Elements/w/datatype/P10314>,
        <http://rdaregistry.info/Elements/w/object/P10314> ;
    reg:lexicalAlias <http://rdaregistry.info/Elements/w/relatedCorporateBodyWork.en> ;
    reg:name "relatedCorporateBodyWork"@en ;
    reg:status <http://metadataregistry.org/uri/RegStatus/1001> ;
    rdfs:domain <http://rdaregistry.info/Elements/c/C10001> ;
    rdfs:isDefinedBy <http://rdaregistry.info/Elements/w/> ;
    rdfs:subPropertyOf <http://rdaregistry.info/Elements/w/P10315> ;
    skos:definition "Relates a work to a corporate body associated with a work being described."@en .

<http://rdaregistry.info/Elements/w/P10316> a rdf:Property ;
    rdfs:label "has related place (work)"@en ;
    reg:hasSubproperty <http://rdaregistry.info/Elements/w/datatype/P10316>,
        <http://rdaregistry.info/Elements/w/object/P10316> ;
    reg:lexicalAlias <http://rdaregistry.info/Elements/w/relatedPlaceWork.en> ;
    reg:name "relatedPlaceWork"@en ;
    reg:status <http://metadataregistry.org/uri/RegStatus/1001> ;
    rdfs:domain <http://rdaregistry.info/Elements/c/C10001> ;
    rdfs:isDefinedBy <http://rdaregistry.info/Elements/w/> ;
    rdfs:subPropertyOf <http://rdaregistry.info/Elements/w/P10307> ;
    skos:definition "Relates a work to a place associated with a work being described."@en .

<http://rdaregistry.info/Elements/w/P10317> a rdf:Property ;
    rdfs:label "has related time-span (work)"@en ;
    reg:hasSubproperty <http://rdaregistry.info/Elements/w/datatype/P10317>,
        <http://rdaregistry.info/Elements/w/object/P10317> ;
    reg:lexicalAlias <http://rdaregistry.info/Elements/w/relatedTimespanWork.en> ;
    reg:name "relatedTimespanWork"@en ;
    reg:status <http://metadataregistry.org/uri/RegStatus/1001> ;
    rdfs:domain <http://rdaregistry.info/Elements/c/C10001> ;
    rdfs:isDefinedBy <http://rdaregistry.info/Elements/w/> ;
    rdfs:subPropertyOf <http://rdaregistry.info/Elements/w/P10307> ;
    skos:definition "Relates a work to a time-span associated with a work being described."@en .

<http://rdaregistry.info/Elements/w/P10318> a rdf:Property ;
    rdfs:label "has related nomen (work)"@en ;
    reg:hasSubproperty <http://rdaregistry.info/Elements/w/datatype/P10318>,
        <http://rdaregistry.info/Elements/w/object/P10318> ;
    reg:lexicalAlias <http://rdaregistry.info/Elements/w/relatedNomenWork.en> ;
    reg:name "relatedNomenWork"@en ;
    reg:status <http://metadataregistry.org/uri/RegStatus/1001> ;
    rdfs:domain <http://rdaregistry.info/Elements/c/C10001> ;
    rdfs:isDefinedBy <http://rdaregistry.info/Elements/w/> ;
    rdfs:subPropertyOf <http://rdaregistry.info/Elements/w/P10307> ;
    skos:definition "Relates a work to a nomen associated with a work being described."@en .

<http://rdaregistry.info/Elements/w/P10321> a rdf:Property ;
    rdfs:label "has subject (place)"@en ;
    reg:hasUnconstrained <http://rdaregistry.info/Elements/u/P60805> ;
    reg:lexicalAlias <http://rdaregistry.info/Elements/w/subjectPlace.en> ;
    reg:name "subjectPlace"@en ;
    reg:status <http://metadataregistry.org/uri/RegStatus/1001> ;
    rdfs:domain <http://rdaregistry.info/Elements/c/C10001> ;
    rdfs:isDefinedBy <http://rdaregistry.info/Elements/w/> ;
    rdfs:subPropertyOf <http://rdaregistry.info/Elements/w/P10256> ;
    skos:definition "Relates a work to a place that a work is about."@en .

<http://rdaregistry.info/Elements/w/P10322> a rdf:Property ;
    rdfs:label "has subject (time-span)"@en ;
    reg:hasUnconstrained <http://rdaregistry.info/Elements/u/P60805> ;
    reg:lexicalAlias <http://rdaregistry.info/Elements/w/subjectTimespan.en> ;
    reg:name "subjectTimespan"@en ;
    reg:status <http://metadataregistry.org/uri/RegStatus/1001> ;
    rdfs:domain <http://rdaregistry.info/Elements/c/C10001> ;
    rdfs:isDefinedBy <http://rdaregistry.info/Elements/w/> ;
    rdfs:subPropertyOf <http://rdaregistry.info/Elements/w/P10256> ;
    skos:definition "Relates a work to a time-span that a work is about."@en .

<http://rdaregistry.info/Elements/w/P10323> a rdf:Property ;
    rdfs:label "has subject (nomen)"@en ;
    reg:hasUnconstrained <http://rdaregistry.info/Elements/u/P60805> ;
    reg:lexicalAlias <http://rdaregistry.info/Elements/w/subjectNomen.en> ;
    reg:name "subjectNomen"@en ;
    reg:status <http://metadataregistry.org/uri/RegStatus/1001> ;
    rdfs:domain <http://rdaregistry.info/Elements/c/C10001> ;
    rdfs:isDefinedBy <http://rdaregistry.info/Elements/w/> ;
    rdfs:subPropertyOf <http://rdaregistry.info/Elements/w/P10256> ;
    skos:definition "Relates a work to a nomen that a work is about."@en .

<http://rdaregistry.info/Elements/w/P10324> a rdf:Property ;
    rdfs:label "has subject (entity)"@en ;
    reg:hasUnconstrained <http://rdaregistry.info/Elements/u/P60805> ;
    reg:lexicalAlias <http://rdaregistry.info/Elements/w/subjectEntity.en> ;
    reg:name "subjectEntity"@en ;
    reg:status <http://metadataregistry.org/uri/RegStatus/1001> ;
    rdfs:domain <http://rdaregistry.info/Elements/c/C10001> ;
    rdfs:isDefinedBy <http://rdaregistry.info/Elements/w/> ;
    skos:definition "Relates a work to an entity that a work is about."@en .

<http://metadataregistry.org/uri/RegStatus/1008> a skos:Concept ;
    skos:prefLabel "Deprecated"@en .

<http://rdaregistry.info/Elements/w/P10001> a rdf:Property ;
    rdfs:label "has respondent"@en ;
    rdakit:instructionNumber "18.5" ;
    rdakit:toolkitDefinition "A candidate for a degree who defends or opposes a thesis provided by the praeses in an academic disputation."@en,
        "Un candidato para un título que defiende o se opone a una tesis proporcionada por los moderadores académicos en un debate académico."@es,
        "Candidat à un diplôme universitaire qui défend ou réfute la thèse proposée par le praeses lors d’une soutenance de thèse."@fr ;
    rdakit:toolkitLabel "respondent"@en,
        "sustentante"@es,
        "répondant"@fr ;
    reg:hasSubproperty <http://rdaregistry.info/Elements/w/object/P10001> ;
    reg:hasUnconstrained <http://rdaregistry.info/Elements/u/P60045> ;
    reg:lexicalAlias <http://rdaregistry.info/Elements/w/respondent.en> ;
    reg:name "respondent"@en ;
    reg:status <http://metadataregistry.org/uri/RegStatus/1001> ;
    rdfs:domain <http://rdaregistry.info/Elements/c/C10001> ;
    rdfs:isDefinedBy <http://rdaregistry.info/Elements/w/> ;
    rdfs:subPropertyOf <http://rdaregistry.info/Elements/w/P10065> ;
    skos:definition "Relates a work to a candidate for a degree who defends or opposes a thesis provided by the praeses in an academic disputation."@en .

<http://rdaregistry.info/Elements/w/P10005> a rdf:Property ;
    rdfs:label "has appellee corporate body"@en ;
    rdakit:instructionNumber "18.5" ;
    rdakit:toolkitDefinition "A corporate body against whom an appeal is taken on a decision of a lower court recorded in a legal work of a higher court."@en,
        "Una entidad corporativa contra la cual se hace una apelación sobre una decisión de una corte menor registrada en una obra jurídica de una corte superior."@es,
        "Collectivité contre laquelle un appel a été formé."@fr ;
    rdakit:toolkitLabel "appellee corporate body"@en,
        "entidad corporativa apelada"@es,
        "collectivité intimée"@fr ;
    reg:hasSubproperty <http://rdaregistry.info/Elements/w/object/P10005> ;
    reg:hasUnconstrained <http://rdaregistry.info/Elements/u/P60373> ;
    reg:lexicalAlias <http://rdaregistry.info/Elements/w/appelleeCorporateBody.en> ;
    reg:name "appelleeCorporateBody"@en ;
    reg:status <http://metadataregistry.org/uri/RegStatus/1001> ;
    rdfs:domain <http://rdaregistry.info/Elements/c/C10001> ;
    rdfs:isDefinedBy <http://rdaregistry.info/Elements/w/> ;
    rdfs:subPropertyOf <http://rdaregistry.info/Elements/w/P10037> ;
    skos:definition "Relates a work to a corporate body against whom an appeal is taken on a decision of a lower court recorded in a legal work of a higher court."@en .

<http://rdaregistry.info/Elements/w/P10006> a rdf:Property ;
    rdfs:label "has degree granting institution"@en ;
    rdakit:instructionNumber "18.5" ;
    rdakit:toolkitDefinition "A corporate body granting an academic degree."@en,
        "Una entidad corporativa que otorga un grado académico."@es,
        "Collectivité conférant un diplôme universitaire."@fr ;
    rdakit:toolkitLabel "degree granting institution"@en,
        "institución que otorga el grado"@es,
        "institution conférant des diplômes universitaires"@fr ;
    reg:hasSubproperty <http://rdaregistry.info/Elements/w/object/P10006> ;
    reg:hasUnconstrained <http://rdaregistry.info/Elements/u/P60060> ;
    reg:lexicalAlias <http://rdaregistry.info/Elements/w/degreeGrantingInstitution.en> ;
    reg:name "degreeGrantingInstitution"@en ;
    reg:status <http://metadataregistry.org/uri/RegStatus/1001> ;
    rdfs:domain <http://rdaregistry.info/Elements/c/C10001> ;
    rdfs:isDefinedBy <http://rdaregistry.info/Elements/w/> ;
    rdfs:subPropertyOf <http://rdaregistry.info/Elements/w/P10047> ;
    skos:definition "Relates a work to a corporate body granting an academic degree."@en .

<http://rdaregistry.info/Elements/w/P10007> a rdf:Property ;
    rdfs:label "has host institution"@en ;
    rdakit:instructionNumber "18.5" ;
    rdakit:toolkitDefinition "A corporate body hosting the event, exhibit, conference, etc., which gave rise to a work, but having little or no responsibility for the content."@en,
        "Una entidad corporativa que es sede de un evento, exposición, conferencia, etc., que da origen a la obra, pero que tiene poca o ninguna responsabilidad por el contenido de la obra."@es,
        "Collectivité accueillant l’événement, l’exposition, le congrès, etc. qui a donné lieu à la création d’une œuvre, mais qui a peu ou pas du tout de responsabilité quant au contenu de l’œuvre."@fr ;
    rdakit:toolkitLabel "host institution"@en,
        "institución sede"@es,
        "institution hôte"@fr ;
    reg:hasSubproperty <http://rdaregistry.info/Elements/w/object/P10007> ;
    reg:hasUnconstrained <http://rdaregistry.info/Elements/u/P60061> ;
    reg:lexicalAlias <http://rdaregistry.info/Elements/w/hostInstitution.en> ;
    reg:name "hostInstitution"@en ;
    reg:status <http://metadataregistry.org/uri/RegStatus/1001> ;
    rdfs:domain <http://rdaregistry.info/Elements/c/C10001> ;
    rdfs:isDefinedBy <http://rdaregistry.info/Elements/w/> ;
    rdfs:subPropertyOf <http://rdaregistry.info/Elements/w/P10047> ;
    skos:definition "Relates a work to a corporate body hosting an event, exhibit, conference, etc., which gave rise to a work, but having little or no responsibility for the content."@en .

<http://rdaregistry.info/Elements/w/P10008> a rdf:Property ;
    rdfs:label "has production company"@en ;
    rdakit:instructionNumber "18.5" ;
    rdakit:toolkitDefinition "A corporate body that is responsible for financial, technical, and organizational management of a production for stage, screen, sound recording, television, webcast, etc."@en,
        "Una entidad corporativa responsable de la gestión financiera, técnica y organizativa de una producción para escena cinematográfica, pantalla, grabación sonora, televisión, emisión web, etc."@es,
        "Collectivité responsable de la gestion financière, technique et organisationnelle de la production d’un spectacle, d’un film, d’un enregistrement audio, d’une émission de télévision, d’une webémission, etc."@fr ;
    rdakit:toolkitLabel "production company"@en,
        "compañía productora"@es,
        "société de production"@fr ;
    reg:hasSubproperty <http://rdaregistry.info/Elements/w/object/P10008> ;
    reg:hasUnconstrained <http://rdaregistry.info/Elements/u/P60062> ;
    reg:lexicalAlias <http://rdaregistry.info/Elements/w/productionCompany.en> ;
    reg:name "productionCompany"@en ;
    reg:status <http://metadataregistry.org/uri/RegStatus/1001> ;
    rdfs:domain <http://rdaregistry.info/Elements/c/C10001> ;
    rdfs:isDefinedBy <http://rdaregistry.info/Elements/w/> ;
    rdfs:subPropertyOf <http://rdaregistry.info/Elements/w/P10047> ;
    skos:definition "Relates a work to a corporate body that is responsible for financial, technical, and organizational management of a production for stage, screen, sound recording, television, webcast, etc."@en .

<http://rdaregistry.info/Elements/w/P10009> a rdf:Property ;
    rdfs:label "has appellant corporate body"@en ;
    rdakit:instructionNumber "18.5" ;
    rdakit:toolkitDefinition "A corporate body who appeals a decision of a lower court recorded in a legal work of a higher court."@en,
        "Una  entidad corporativa que apela una decisión de una corte menor registrada en una obra jurídica de una corte superior."@es,
        "Collectivité qui en appelle de la décision d’un tribunal inférieur."@fr ;
    rdakit:toolkitLabel "appellant corporate body"@en,
        "entidad corporativa apelante"@es,
        "collectivité appelante"@fr ;
    reg:hasSubproperty <http://rdaregistry.info/Elements/w/object/P10009> ;
    reg:hasUnconstrained <http://rdaregistry.info/Elements/u/P60457> ;
    reg:lexicalAlias <http://rdaregistry.info/Elements/w/appellantCorporateBody.en> ;
    reg:name "appellantCorporateBody"@en ;
    reg:status <http://metadataregistry.org/uri/RegStatus/1001> ;
    rdfs:domain <http://rdaregistry.info/Elements/c/C10001> ;
    rdfs:isDefinedBy <http://rdaregistry.info/Elements/w/> ;
    rdfs:subPropertyOf <http://rdaregistry.info/Elements/w/P10038> ;
    skos:definition "Relates a work to a corporate body who appeals a decision of a lower court recorded in a legal work of a higher court."@en .

<http://rdaregistry.info/Elements/w/P10010> a rdf:Property ;
    rdfs:label "has plaintiff corporate body"@en ;
    rdakit:instructionNumber "18.5" ;
    rdakit:toolkitDefinition "A corporate body who brings a suit in a civil proceeding."@en,
        "Una entidad corporativa que presenta una demanda en un proceso civil."@es,
        "Collectivité qui intente une poursuite civile."@fr ;
    rdakit:toolkitLabel "plaintiff corporate body"@en,
        "entidad corporativa demandante"@es,
        "collectivité demanderesse"@fr ;
    reg:hasSubproperty <http://rdaregistry.info/Elements/w/object/P10010> ;
    reg:hasUnconstrained <http://rdaregistry.info/Elements/u/P60459> ;
    reg:lexicalAlias <http://rdaregistry.info/Elements/w/plaintiffCorporateBody.en> ;
    reg:name "plaintiffCorporateBody"@en ;
    reg:status <http://metadataregistry.org/uri/RegStatus/1001> ;
    rdfs:domain <http://rdaregistry.info/Elements/c/C10001> ;
    rdfs:isDefinedBy <http://rdaregistry.info/Elements/w/> ;
    rdfs:subPropertyOf <http://rdaregistry.info/Elements/w/P10039> ;
    skos:definition "Relates a work to a corporate body who brings a suit in a civil proceeding."@en .

<http://rdaregistry.info/Elements/w/P10011> a rdf:Property ;
    rdfs:label "has court governed"@en ;
    rdakit:instructionNumber "18.5" ;
    rdakit:toolkitDefinition "A court governed by court rules, regardless of their official nature."@en,
        "Un tribunal regido por reglamentos de tribunales, independientemente de su naturaleza oficial (por ej., leyes, disposiciones administrativas)."@es,
        "Tribunal régi par des règles de pratique, sans égard à leur nature officielle (par exemple, lois, règlements)."@fr ;
    rdakit:toolkitLabel "court governed"@en,
        "tribunal regido"@es,
        "tribunal régi"@fr ;
    reg:hasSubproperty <http://rdaregistry.info/Elements/w/object/P10011> ;
    reg:hasUnconstrained <http://rdaregistry.info/Elements/u/P60065> ;
    reg:lexicalAlias <http://rdaregistry.info/Elements/w/courtGoverned.en> ;
    reg:name "courtGoverned"@en ;
    reg:status <http://metadataregistry.org/uri/RegStatus/1001> ;
    rdfs:domain <http://rdaregistry.info/Elements/c/C10001> ;
    rdfs:isDefinedBy <http://rdaregistry.info/Elements/w/> ;
    rdfs:subPropertyOf <http://rdaregistry.info/Elements/w/P10047> ;
    skos:definition "Relates a work to a court governed by court rules, regardless of their official nature."@en .

<http://rdaregistry.info/Elements/w/P10013> a rdf:Property ;
    rdfs:label "has film director"@en ;
    rdakit:instructionNumber "18.5" ;
    rdakit:toolkitDefinition "A director responsible for the general management and supervision of a filmed performance."@en,
        "Un director responsable de la gestión y supervisión general de una producción cinematográfica."@es,
        "Réalisateur responsable de la gestion et de la supervision générales d’une prestation filmée."@fr ;
    rdakit:toolkitLabel "film director"@en,
        "director de cine"@es,
        "réalisateur de films"@fr ;
    reg:hasSubproperty <http://rdaregistry.info/Elements/w/object/P10013> ;
    reg:hasUnconstrained <http://rdaregistry.info/Elements/u/P60084> ;
    reg:lexicalAlias <http://rdaregistry.info/Elements/w/filmDirector.en> ;
    reg:name "filmDirector"@en ;
    reg:status <http://metadataregistry.org/uri/RegStatus/1001> ;
    rdfs:domain <http://rdaregistry.info/Elements/c/C10001> ;
    rdfs:isDefinedBy <http://rdaregistry.info/Elements/w/> ;
    rdfs:subPropertyOf <http://rdaregistry.info/Elements/w/P10066> ;
    skos:definition "Relates a work to a director responsible for the general management and supervision of a filmed performance."@en .

<http://rdaregistry.info/Elements/w/P10014> a rdf:Property ;
    rdfs:label "has radio director"@en ;
    rdakit:instructionNumber "18.5" ;
    rdakit:toolkitDefinition "A director responsible for the general management and supervision of a radio program."@en,
        "Un director responsable de la dirección y supervisión general de un programa de radio."@es,
        "Réalisateur responsable de la gestion et de la supervision générales d’une émission de radio."@fr ;
    rdakit:toolkitLabel "radio director"@en,
        "director de radio"@es,
        "réalisateur d’émissions de radio"@fr ;
    reg:hasSubproperty <http://rdaregistry.info/Elements/w/object/P10014> ;
    reg:hasUnconstrained <http://rdaregistry.info/Elements/u/P60085> ;
    reg:lexicalAlias <http://rdaregistry.info/Elements/w/radioDirector.en> ;
    reg:name "radioDirector"@en ;
    reg:status <http://metadataregistry.org/uri/RegStatus/1001> ;
    rdfs:domain <http://rdaregistry.info/Elements/c/C10001> ;
    rdfs:isDefinedBy <http://rdaregistry.info/Elements/w/> ;
    rdfs:subPropertyOf <http://rdaregistry.info/Elements/w/P10066> ;
    skos:definition "Relates a work to a director responsible for the general management and supervision of a radio program."@en .

<http://rdaregistry.info/Elements/w/P10015> a rdf:Property ;
    rdfs:label "has television director"@en ;
    rdakit:instructionNumber "18.5" ;
    rdakit:toolkitDefinition "A director responsible for the general management and supervision of a television program."@en,
        "Un director responsable por la dirección y supervisión general de un programa de televisión."@es,
        "Réalisateur responsable de la gestion et de la supervision générales d’une émission de télévision."@fr ;
    rdakit:toolkitLabel "television director"@en,
        "director de televisión"@es,
        "réalisateur d’émissions de télévision"@fr ;
    reg:hasSubproperty <http://rdaregistry.info/Elements/w/object/P10015> ;
    reg:hasUnconstrained <http://rdaregistry.info/Elements/u/P60086> ;
    reg:lexicalAlias <http://rdaregistry.info/Elements/w/televisionDirector.en> ;
    reg:name "televisionDirector"@en ;
    reg:status <http://metadataregistry.org/uri/RegStatus/1001> ;
    rdfs:domain <http://rdaregistry.info/Elements/c/C10001> ;
    rdfs:isDefinedBy <http://rdaregistry.info/Elements/w/> ;
    rdfs:subPropertyOf <http://rdaregistry.info/Elements/w/P10066> ;
    skos:definition "Relates a work to a director responsible for the general management and supervision of a television program."@en .

<http://rdaregistry.info/Elements/w/P10016> a rdf:Property ;
    rdfs:label "is dramatized as (work)"@en ;
    rdakit:instructionNumber "24.5" ;
    rdakit:toolkitDefinition "A dramatic work adapted from a source work."@en,
        "Una obra dramática adaptada de la obra fuente."@es,
        "Œuvre théâtrale adaptée de l’œuvre source."@fr ;
    rdakit:toolkitLabel "dramatized as (work)"@en,
        "dramatizada como (obra)"@es,
        "adapté au théâtre comme (œuvre)"@fr ;
    reg:hasSubproperty <http://rdaregistry.info/Elements/w/object/P10016> ;
    reg:hasUnconstrained <http://rdaregistry.info/Elements/u/P60088> ;
    reg:lexicalAlias <http://rdaregistry.info/Elements/w/dramatizedAsWork.en> ;
    reg:name "dramatizedAsWork"@en ;
    reg:status <http://metadataregistry.org/uri/RegStatus/1001> ;
    rdfs:domain <http://rdaregistry.info/Elements/c/C10001> ;
    rdfs:isDefinedBy <http://rdaregistry.info/Elements/w/> ;
    rdfs:subPropertyOf <http://rdaregistry.info/Elements/w/P10155> ;
    skos:definition "Relates a work to a dramatic work adapted from a source work."@en .

<http://rdaregistry.info/Elements/w/P10017> a rdf:Property ;
    rdfs:label "has enacting jurisdiction"@en ;
    rdakit:instructionNumber "18.5" ;
    rdakit:toolkitDefinition "A jurisdiction enacting a law, regulation, constitution, court rule, etc."@en,
        "Una jurisdicción que promulga una ley, disposición, constitución, reglamento de tribunal, etc."@es,
        "Juridiction promulguant une loi, un règlement, une constitution, une règle de pratique de tribunal, etc."@fr ;
    rdakit:toolkitLabel "enacting jurisdiction"@en,
        "jurisdicción promulgadora"@es,
        "juridiction promulgatrice"@fr ;
    reg:hasSubproperty <http://rdaregistry.info/Elements/w/object/P10017> ;
    reg:hasUnconstrained <http://rdaregistry.info/Elements/u/P60096> ;
    reg:lexicalAlias <http://rdaregistry.info/Elements/w/enactingJurisdiction.en> ;
    reg:name "enactingJurisdiction"@en ;
    reg:status <http://metadataregistry.org/uri/RegStatus/1001> ;
    rdfs:domain <http://rdaregistry.info/Elements/c/C10001> ;
    rdfs:isDefinedBy <http://rdaregistry.info/Elements/w/> ;
    rdfs:subPropertyOf <http://rdaregistry.info/Elements/w/P10065> ;
    skos:definition "Relates a work to a jurisdiction enacting a law, regulation, constitution, court rule, etc."@en .

<http://rdaregistry.info/Elements/w/P10018> a rdf:Property ;
    rdfs:label "has jurisdiction governed"@en ;
    rdakit:instructionNumber "18.5" ;
    rdakit:toolkitDefinition "A jurisdiction governed by a law, regulation, etc., that was enacted by another jurisdiction."@en,
        "Una jurisdicción en la que se aplica una ley, disposición, etc., que fue promulgada por otra jurisdicción."@es,
        "Juridiction régie par une loi, un règlement, etc. qui a été promulgué par une autre juridiction."@fr ;
    rdakit:toolkitLabel "jurisdiction governed"@en,
        "jurisdicción regulada"@es,
        "juridiction régie"@fr ;
    reg:hasSubproperty <http://rdaregistry.info/Elements/w/object/P10018> ;
    reg:hasUnconstrained <http://rdaregistry.info/Elements/u/P60097> ;
    reg:lexicalAlias <http://rdaregistry.info/Elements/w/jurisdictionGoverned.en> ;
    reg:name "jurisdictionGoverned"@en ;
    reg:status <http://metadataregistry.org/uri/RegStatus/1001> ;
    rdfs:domain <http://rdaregistry.info/Elements/c/C10001> ;
    rdfs:isDefinedBy <http://rdaregistry.info/Elements/w/> ;
    rdfs:subPropertyOf <http://rdaregistry.info/Elements/w/P10047> ;
    skos:definition "Relates a work to a jurisdiction governed by a law, regulation, etc., that was enacted by another jurisdiction."@en .

<http://rdaregistry.info/Elements/w/P10020> a rdf:Property ;
    rdfs:label "is sequel"@en ;
    rdakit:instructionNumber "24.5" ;
    rdakit:toolkitDefinition "A later work that continues the narrative of an earlier work."@en,
        "Una obra posterior que continúa la narración de una obra anterior."@es,
        "Œuvre ultérieure qui continue le récit d’une œuvre antérieure."@fr ;
    rdakit:toolkitLabel "sequel"@en,
        "secuela"@es,
        "suite"@fr ;
    reg:hasSubproperty <http://rdaregistry.info/Elements/w/object/P10020> ;
    reg:hasUnconstrained <http://rdaregistry.info/Elements/u/P60102> ;
    reg:lexicalAlias <http://rdaregistry.info/Elements/w/sequel.en> ;
    reg:name "sequel"@en ;
    reg:status <http://metadataregistry.org/uri/RegStatus/1001> ;
    rdfs:domain <http://rdaregistry.info/Elements/c/C10001> ;
    rdfs:isDefinedBy <http://rdaregistry.info/Elements/w/> ;
    rdfs:subPropertyOf <http://rdaregistry.info/Elements/w/P10170> ;
    skos:definition "Relates a work to a later work that continues the narrative of an earlier work."@en .

<http://rdaregistry.info/Elements/w/P10021> a rdf:Property ;
    rdfs:label "is replaced in part by (work)"@en ;
    rdakit:instructionNumber "24.5" ;
    rdakit:toolkitDefinition "A later work used in part in place of an earlier work, usually because the later work contains updated or new information that makes part of the earlier work obsolete."@en,
        "Una obra posterior usada en parte en lugar de una obra anterior, generalmente porque la obra posterior contiene información actualizada o nueva que hace obsoleta parte de la obra anterior."@es,
        "Œuvre ultérieure utilisée en partie à la place d’une œuvre antérieure, généralement parce que l’œuvre ultérieure contient de l’information nouvelle ou mise à jour qui rend une partie de l’œuvre antérieure obsolète."@fr ;
    rdakit:toolkitLabel "replaced in part by (work)"@en,
        "reemplazada en parte por (obra)"@es,
        "remplacé en partie par (œuvre)"@fr ;
    reg:hasSubproperty <http://rdaregistry.info/Elements/w/object/P10021> ;
    reg:hasUnconstrained <http://rdaregistry.info/Elements/u/P60103> ;
    reg:lexicalAlias <http://rdaregistry.info/Elements/w/replacedInPartByWork.en> ;
    reg:name "replacedInPartByWork"@en ;
    reg:status <http://metadataregistry.org/uri/RegStatus/1001> ;
    rdfs:domain <http://rdaregistry.info/Elements/c/C10001> ;
    rdfs:isDefinedBy <http://rdaregistry.info/Elements/w/> ;
    rdfs:subPropertyOf <http://rdaregistry.info/Elements/w/P10170> ;
    skos:definition "Relates a work to a later work used in part in place of an earlier work, usually because the later work contains updated or new information that makes part of the earlier work obsolete."@en ;
    skos:scopeNote "This relationship applies generally to single-part units, multipart monographs, and integrating resources."@en .

<http://rdaregistry.info/Elements/w/P10022> a rdf:Property ;
    rdfs:label "is replaced by (work)"@en ;
    rdakit:instructionNumber "24.5" ;
    rdakit:toolkitDefinition "A later work used in place of an earlier work, usually because the later work contains updated or new information that makes the earlier work obsolete."@en,
        "Una obra posterior usada en lugar de una obra anterior, generalmente porque la obra posterior contiene información actualizada o nueva que hace obsoleta la obra anterior."@es,
        "Œuvre ultérieure utilisée à la place d’une œuvre antérieure, généralement parce que l’œuvre ultérieure contient de l’information nouvelle ou mise à jour qui rend l’œuvre antérieure obsolète."@fr ;
    rdakit:toolkitLabel "replaced by (work)"@en,
        "reemplazada por (obra)"@es,
        "remplacé par (œuvre)"@fr ;
    reg:hasSubproperty <http://rdaregistry.info/Elements/w/object/P10022> ;
    reg:hasUnconstrained <http://rdaregistry.info/Elements/u/P60104> ;
    reg:lexicalAlias <http://rdaregistry.info/Elements/w/replacedByWork.en> ;
    reg:name "replacedByWork"@en ;
    reg:status <http://metadataregistry.org/uri/RegStatus/1001> ;
    rdfs:domain <http://rdaregistry.info/Elements/c/C10001> ;
    rdfs:isDefinedBy <http://rdaregistry.info/Elements/w/> ;
    rdfs:subPropertyOf <http://rdaregistry.info/Elements/w/P10170> ;
    skos:definition "Relates a work to a later work used in place of an earlier work, usually because the later work contains updated or new information that makes the earlier work obsolete."@en ;
    skos:scopeNote "This relationship applies generally to single-part units, multipart monographs, and integrating resources."@en .

<http://rdaregistry.info/Elements/w/P10023> a rdf:Property ;
    rdfs:label "is adapted in verse as (work)"@en ;
    rdakit:instructionNumber "24.5" ;
    rdakit:toolkitDefinition "A literary composition in verse form adapted from a source work."@en,
        "Una composición literaria en verso adaptada de la obra fuente."@es,
        "Composition littéraire en vers adaptée de l’œuvre source."@fr ;
    rdakit:toolkitLabel "adapted in verse as (work)"@en,
        "adaptada en verso como (obra)"@es,
        "adapté en vers comme (œuvre)"@fr ;
    reg:hasSubproperty <http://rdaregistry.info/Elements/w/object/P10023> ;
    reg:hasUnconstrained <http://rdaregistry.info/Elements/u/P60106> ;
    reg:lexicalAlias <http://rdaregistry.info/Elements/w/adaptedInVerseAsWork.en> ;
    reg:name "adaptedInVerseAsWork"@en ;
    reg:status <http://metadataregistry.org/uri/RegStatus/1001> ;
    rdfs:domain <http://rdaregistry.info/Elements/c/C10001> ;
    rdfs:isDefinedBy <http://rdaregistry.info/Elements/w/> ;
    rdfs:subPropertyOf <http://rdaregistry.info/Elements/w/P10155> ;
    skos:definition "Relates a work to a literary composition in verse form adapted from a source work."@en .

<http://rdaregistry.info/Elements/w/P10025> a rdf:Property ;
    rdfs:label "is adapted as motion picture (work)"@en ;
    rdakit:instructionNumber "24.5" ;
    rdakit:toolkitDefinition "A motion picture based on a source work."@en,
        "Una película cinematográfica basada en la obra fuente."@es,
        "Film basé sur l’œuvre source."@fr ;
    rdakit:toolkitLabel "adapted as motion picture (work)"@en,
        "adaptada como película cinematográfica (obra)"@es,
        "adapté en film (œuvre)"@fr ;
    reg:hasSubproperty <http://rdaregistry.info/Elements/w/object/P10025> ;
    reg:hasUnconstrained <http://rdaregistry.info/Elements/u/P60110> ;
    reg:lexicalAlias <http://rdaregistry.info/Elements/w/adaptedAsMotionPictureWork.en> ;
    reg:name "adaptedAsMotionPictureWork"@en ;
    reg:status <http://metadataregistry.org/uri/RegStatus/1001> ;
    rdfs:domain <http://rdaregistry.info/Elements/c/C10001> ;
    rdfs:isDefinedBy <http://rdaregistry.info/Elements/w/> ;
    rdfs:subPropertyOf <http://rdaregistry.info/Elements/w/P10155> ;
    skos:definition "Relates a work to a motion picture based on a source work."@en .

<http://rdaregistry.info/Elements/w/P10026> a rdf:Property ;
    rdfs:label "is cadenza (work)"@en ;
    rdakit:instructionNumber "24.5" ;
    rdakit:toolkitDefinition "A musical work consisting of an ornamental passage for a soloist, added to a musical work such as a concerto, either by the same or a different composer."@en,
        "Una obra musical que consiste en un pasaje ornamental para solista, agregada a una obra musical como un concierto, por igual o diferente compositor."@es,
        "Œuvre musicale consistant en un passage ornemental pour soliste, ajouté à une œuvre musicale telle qu’un concerto, soit par le même compositeur, soit par un compositeur différent."@fr ;
    rdakit:toolkitLabel "cadenza (work)"@en,
        "cadencia (obra)"@es,
        "cadence (œuvre)"@fr ;
    reg:hasSubproperty <http://rdaregistry.info/Elements/w/object/P10026> ;
    reg:hasUnconstrained <http://rdaregistry.info/Elements/u/P60113> ;
    reg:lexicalAlias <http://rdaregistry.info/Elements/w/cadenzaWork.en> ;
    reg:name "cadenzaWork"@en ;
    reg:status <http://metadataregistry.org/uri/RegStatus/1001> ;
    rdfs:domain <http://rdaregistry.info/Elements/c/C10001> ;
    rdfs:isDefinedBy <http://rdaregistry.info/Elements/w/> ;
    rdfs:subPropertyOf <http://rdaregistry.info/Elements/w/P10108> ;
    skos:definition "Relates a work to a musical work consisting of an ornamental passage for a soloist, added to a musical work such as a concerto, either by the same or a different composer."@en .

<http://rdaregistry.info/Elements/w/P10027> a rdf:Property ;
    rdfs:label "is variations based on (work)"@en ;
    rdakit:instructionNumber "24.5" ;
    rdakit:toolkitDefinition "A musical work from which melodic, thematic, or harmonic material is taken to form a discrete theme, which is repeated one or more times with subsequent modifications."@en,
        "Una obra musical de la cual se toma material melódico, temático o armónico para formar un tema separado, que se repite una o más veces con modificaciones subsecuentes."@es,
        "Œuvre musicale d’où est tirée de la matière mélodique, thématique ou harmonique pour former un thème distinct, qui est répété une ou plusieurs fois avec des modifications subséquentes."@fr ;
    rdakit:toolkitLabel "variations based on (work)"@en,
        "variaciones basadas en (obra)"@es,
        "variations basées sur (œuvre)"@fr ;
    reg:hasSubproperty <http://rdaregistry.info/Elements/w/object/P10027> ;
    reg:hasUnconstrained <http://rdaregistry.info/Elements/u/P60114> ;
    reg:lexicalAlias <http://rdaregistry.info/Elements/w/variationsBasedOnWork.en> ;
    reg:name "variationsBasedOnWork"@en ;
    reg:status <http://metadataregistry.org/uri/RegStatus/1001> ;
    rdfs:domain <http://rdaregistry.info/Elements/c/C10001> ;
    rdfs:isDefinedBy <http://rdaregistry.info/Elements/w/> ;
    rdfs:subPropertyOf <http://rdaregistry.info/Elements/w/P10190> ;
    skos:definition "Relates a work to a musical work from which melodic, thematic, or harmonic material is taken to form a discrete theme, which is repeated one or more times with subsequent modifications."@en .

<http://rdaregistry.info/Elements/w/P10028> a rdf:Property ;
    rdfs:label "is modified by variation as (work)"@en ;
    rdakit:instructionNumber "24.5" ;
    rdakit:toolkitDefinition "A musical work in which melodic, thematic, or harmonic material taken from a source work forms a discrete theme, which is repeated one or more times with subsequent modifications."@en,
        "Una obra musical en la cual el material melódico, temático o armónico de la obra fuente se toma para formar un tema separado, el cual se repite una o más veces con modificaciones subsecuentes"@es,
        "Œuvre musicale dans laquelle de la matière mélodique, thématique ou harmonique tirée de l’œuvre source forme un thème distinct qui est répété une ou plusieurs fois avec des modifications subséquentes."@fr ;
    rdakit:toolkitLabel "modified by variation as (work)"@en,
        "modificada por variación como (obra)"@es,
        "modifié par variation comme (œuvre)"@fr ;
    reg:hasSubproperty <http://rdaregistry.info/Elements/w/object/P10028> ;
    reg:hasUnconstrained <http://rdaregistry.info/Elements/u/P60115> ;
    reg:lexicalAlias <http://rdaregistry.info/Elements/w/modifiedByVariationAsWork.en> ;
    reg:name "modifiedByVariationAsWork"@en ;
    reg:status <http://metadataregistry.org/uri/RegStatus/1001> ;
    rdfs:domain <http://rdaregistry.info/Elements/c/C10001> ;
    rdfs:isDefinedBy <http://rdaregistry.info/Elements/w/> ;
    rdfs:subPropertyOf <http://rdaregistry.info/Elements/w/P10148> ;
    skos:definition "Relates a work to a musical work in which melodic, thematic, or harmonic material taken from a source work forms a discrete theme, which is repeated one or more times with subsequent modifications."@en .

<http://rdaregistry.info/Elements/w/P10029> a rdf:Property ;
    rdfs:label "is cadenza composed for (work)"@en ;
    rdakit:instructionNumber "24.5" ;
    rdakit:toolkitDefinition "A musical work such as a concerto for which an ornamental passage for a soloist has been composed, either by the same or a different composer."@en,
        "Una obra musical como un concierto para el cual se compuso un pasaje ornamental para solista, por igual o diferente compositor."@es,
        "Œuvre musicale telle qu’un concerto pour laquelle un passage ornemental pour soliste a été composé, soit par le même compositeur, soit par un compositeur différent."@fr ;
    rdakit:toolkitLabel "cadenza composed for (work)"@en,
        "cadencia compuesta para (obra)"@es,
        "cadence composée pour (œuvre)"@fr ;
    reg:hasSubproperty <http://rdaregistry.info/Elements/w/object/P10029> ;
    reg:hasUnconstrained <http://rdaregistry.info/Elements/u/P60116> ;
    reg:lexicalAlias <http://rdaregistry.info/Elements/w/cadenzaComposedForWork.en> ;
    reg:name "cadenzaComposedForWork"@en ;
    reg:status <http://metadataregistry.org/uri/RegStatus/1001> ;
    rdfs:domain <http://rdaregistry.info/Elements/c/C10001> ;
    rdfs:isDefinedBy <http://rdaregistry.info/Elements/w/> ;
    rdfs:subPropertyOf <http://rdaregistry.info/Elements/w/P10192> ;
    skos:definition "Relates a work to a musical work such as a concerto for which an ornamental passage for a soloist has been composed, either by the same or a different composer."@en .

<http://rdaregistry.info/Elements/w/P10030> a rdf:Property ;
    rdfs:label "is libretto for (work)"@en ;
    rdakit:instructionNumber "24.5" ;
    rdakit:toolkitDefinition "A musical work such as an opera or other work for the musical stage, or an oratorio, that uses the text of a related work."@en,
        "Una obra musical tal como una ópera u otra obra para representación musical o un oratorio, que utiliza el texto de la obra relacionada como libreto."@es,
        "Œuvre musicale telle qu’un opéra ou une autre œuvre pour la scène musicale, ou telle qu’un oratorio, qui utilise le texte de l’œuvre en relation comme livret."@fr ;
    rdakit:toolkitLabel "libretto for (work)"@en,
        "libreto para (obra)"@es,
        "livret pour (œuvre)"@fr ;
    reg:hasSubproperty <http://rdaregistry.info/Elements/w/object/P10030> ;
    reg:hasUnconstrained <http://rdaregistry.info/Elements/u/P60117> ;
    reg:lexicalAlias <http://rdaregistry.info/Elements/w/librettoForWork.en> ;
    reg:name "librettoForWork"@en ;
    reg:status <http://metadataregistry.org/uri/RegStatus/1001> ;
    rdfs:domain <http://rdaregistry.info/Elements/c/C10001> ;
    rdfs:isDefinedBy <http://rdaregistry.info/Elements/w/> ;
    rdfs:subPropertyOf <http://rdaregistry.info/Elements/w/P10103> ;
    skos:definition "Relates a work to a musical work such as an opera or other work for the musical stage, or an oratorio, that uses the text of a related work."@en .

<http://rdaregistry.info/Elements/w/P10031> a rdf:Property ;
    rdfs:label "is incidental music (work)"@en ;
    rdakit:instructionNumber "24.5" ;
    rdakit:toolkitDefinition "A musical work that provides incidental music for a play or other spoken work for the stage."@en,
        "Una obra musical que proporciona música incidental para una obra de teatro u otra obra hablada para el escenario."@es,
        "Œuvre musicale qui fournit la musique de scène pour une pièce de théâtre ou une autre œuvre parlée pour la scène."@fr ;
    rdakit:toolkitLabel "incidental music (work)"@en,
        "música incidental (obra)"@es,
        "musique de scène (œuvre)"@fr ;
    reg:hasSubproperty <http://rdaregistry.info/Elements/w/object/P10031> ;
    reg:hasUnconstrained <http://rdaregistry.info/Elements/u/P60118> ;
    reg:lexicalAlias <http://rdaregistry.info/Elements/w/incidentalMusicWork.en> ;
    reg:name "incidentalMusicWork"@en ;
    reg:status <http://metadataregistry.org/uri/RegStatus/1001> ;
    rdfs:domain <http://rdaregistry.info/Elements/c/C10001> ;
    rdfs:isDefinedBy <http://rdaregistry.info/Elements/w/> ;
    rdfs:subPropertyOf <http://rdaregistry.info/Elements/w/P10237> ;
    skos:definition "Relates a work to a musical work that provides incidental music for a play or other spoken work for the stage."@en .

<http://rdaregistry.info/Elements/w/P10032> a rdf:Property ;
    rdfs:label "is remade as (work)"@en ;
    rdakit:instructionNumber "24.5" ;
    rdakit:toolkitDefinition "A new motion picture, radio program, television program, or video based on an earlier work."@en,
        "Una película cinematográfica, un programa de radio, televisión o video nuevo basados en una obra anterior."@es,
        "Nouveau film, nouvelle émission de radio, nouvelle émission de télévision ou nouvelle vidéo basée sur une œuvre antérieure."@fr ;
    rdakit:toolkitLabel "remade as (work)"@en,
        "reproducida como (obra)"@es,
        "repris comme (œuvre)"@fr ;
    reg:hasSubproperty <http://rdaregistry.info/Elements/w/object/P10032> ;
    reg:hasUnconstrained <http://rdaregistry.info/Elements/u/P60120> ;
    reg:lexicalAlias <http://rdaregistry.info/Elements/w/remadeAsWork.en> ;
    reg:name "remadeAsWork"@en ;
    reg:status <http://metadataregistry.org/uri/RegStatus/1001> ;
    rdfs:domain <http://rdaregistry.info/Elements/c/C10001> ;
    rdfs:isDefinedBy <http://rdaregistry.info/Elements/w/> ;
    rdfs:subPropertyOf <http://rdaregistry.info/Elements/w/P10148> ;
    skos:definition "Relates a work to a motion picture, radio program, television program, or video based on an earlier work."@en .

<http://rdaregistry.info/Elements/w/P10033> a rdf:Property ;
    rdfs:label "is set to music as (work)"@en ;
    rdakit:instructionNumber "24.5" ;
    rdakit:toolkitDefinition "A non-dramatic musical work, other than an oratorio, that uses the text of a source work."@en,
        "Una obra musical no dramática, diferente del oratorio, que usa el texto de la obra fuente."@es,
        "Œuvre musicale non théâtrale, autre qu’un oratorio, qui utilise le texte de l’œuvre source."@fr ;
    rdakit:toolkitLabel "set to music as (work)"@en,
        "hecha para música como (obra)"@es,
        "mis en musique comme (œuvre)"@fr ;
    reg:hasSubproperty <http://rdaregistry.info/Elements/w/object/P10033> ;
    reg:hasUnconstrained <http://rdaregistry.info/Elements/u/P60121> ;
    reg:lexicalAlias <http://rdaregistry.info/Elements/w/setToMusicAsWork.en> ;
    reg:name "setToMusicAsWork"@en ;
    reg:status <http://metadataregistry.org/uri/RegStatus/1001> ;
    rdfs:domain <http://rdaregistry.info/Elements/c/C10001> ;
    rdfs:isDefinedBy <http://rdaregistry.info/Elements/w/> ;
    rdfs:subPropertyOf <http://rdaregistry.info/Elements/w/P10148> ;
    skos:definition "Relates a work to a non-dramatic musical work, other than an oratorio, that uses the text of a source work."@en .

<http://rdaregistry.info/Elements/w/P10034> a rdf:Property ;
    rdfs:label "is adapted as novel (work)"@en ;
    rdakit:instructionNumber "24.5" ;
    rdakit:toolkitDefinition "A novel adapted from a source work."@en,
        "Una novela adaptada de la obra fuente."@es,
        "Roman adapté de l’œuvre source."@fr ;
    rdakit:toolkitLabel "adapted as novel (work)"@en,
        "adaptada como novela (obra)"@es,
        "adapté en roman (œuvre)"@fr ;
    reg:hasSubproperty <http://rdaregistry.info/Elements/w/object/P10034> ;
    reg:hasUnconstrained <http://rdaregistry.info/Elements/u/P60138> ;
    reg:lexicalAlias <http://rdaregistry.info/Elements/w/adaptedAsNovelWork.en> ;
    reg:name "adaptedAsNovelWork"@en ;
    reg:status <http://metadataregistry.org/uri/RegStatus/1001> ;
    rdfs:domain <http://rdaregistry.info/Elements/c/C10001> ;
    rdfs:isDefinedBy <http://rdaregistry.info/Elements/w/> ;
    rdfs:subPropertyOf <http://rdaregistry.info/Elements/w/P10155> ;
    skos:definition "Relates a work to a novel adapted from a source work."@en .

<http://rdaregistry.info/Elements/w/P10035> a rdf:Property ;
    rdfs:label "has appellee person"@en ;
    rdakit:instructionNumber "18.5" ;
    rdakit:toolkitDefinition "A person against whom an appeal is taken on a decision of a lower court recorded in a legal work of a higher court."@en,
        "Una persona contra la cual se hace una apelación sobre una decisión de una corte menor registrada en una obra jurídica de una corte superior."@es,
        "Personne contre laquelle un appel a été formé."@fr ;
    rdakit:toolkitLabel "appellee person"@en,
        "persona apelada"@es,
        "personne intimée"@fr ;
    reg:hasSubproperty <http://rdaregistry.info/Elements/w/object/P10035> ;
    reg:hasUnconstrained <http://rdaregistry.info/Elements/u/P60373> ;
    reg:lexicalAlias <http://rdaregistry.info/Elements/w/appelleePerson.en> ;
    reg:name "appelleePerson"@en ;
    reg:status <http://metadataregistry.org/uri/RegStatus/1001> ;
    rdfs:domain <http://rdaregistry.info/Elements/c/C10001> ;
    rdfs:isDefinedBy <http://rdaregistry.info/Elements/w/> ;
    rdfs:subPropertyOf <http://rdaregistry.info/Elements/w/P10037> ;
    skos:definition "Relates a work to a person against whom an appeal is taken on a decision of a lower court recorded in a legal work of a higher court."@en .

<http://rdaregistry.info/Elements/w/P10036> a rdf:Property ;
    rdfs:label "has medium"@en ;
    rdakit:instructionNumber "18.5" ;
    rdakit:toolkitDefinition "A person held to be a channel of communication between the earthly world and a world of spirits."@en,
        "Una persona tenida como una canal de comunicación entre el mundo terrenal y el mundo de los espíritus."@es,
        "Personne tenue pour être un canal de communication entre le monde terrestre et le monde des esprits."@fr ;
    rdakit:toolkitLabel "medium"@en,
        "médium"@es,
        "médium"@fr ;
    reg:hasSubproperty <http://rdaregistry.info/Elements/w/object/P10036> ;
    reg:hasUnconstrained <http://rdaregistry.info/Elements/u/P60157> ;
    reg:lexicalAlias <http://rdaregistry.info/Elements/w/medium.en> ;
    reg:name "medium"@en ;
    reg:status <http://metadataregistry.org/uri/RegStatus/1001> ;
    rdfs:domain <http://rdaregistry.info/Elements/c/C10001> ;
    rdfs:isDefinedBy <http://rdaregistry.info/Elements/w/> ;
    rdfs:subPropertyOf <http://rdaregistry.info/Elements/w/P10047> ;
    skos:definition "Relates a work to a person held to be a channel of communication between the earthly world and a world of spirits."@en .

<http://rdaregistry.info/Elements/w/P10041> a rdf:Property ;
    rdfs:label "has degree supervisor"@en ;
    rdakit:instructionNumber "18.5" ;
    rdakit:toolkitDefinition "A person, such as an advisor or supervisor of thesis or dissertation research, overseeing either an academic degree or thesis."@en,
        "Una persona, tal como un director o supervisor de tesis de grado o investigación, que supervisa un grado académico o tesis."@es,
        "Personne supervisant un diplôme universitaire de niveau supérieur."@fr ;
    rdakit:toolkitLabel "degree supervisor"@en,
        "supervisor de grado"@es,
        "superviseur académique"@fr ;
    reg:hasSubproperty <http://rdaregistry.info/Elements/w/object/P10041> ;
    reg:hasUnconstrained <http://rdaregistry.info/Elements/u/P60420> ;
    reg:lexicalAlias <http://rdaregistry.info/Elements/w/degreeSupervisor.en> ;
    reg:name "degreeSupervisor"@en ;
    reg:status <http://metadataregistry.org/uri/RegStatus/1001> ;
    rdfs:domain <http://rdaregistry.info/Elements/c/C10001> ;
    rdfs:isDefinedBy <http://rdaregistry.info/Elements/w/> ;
    rdfs:subPropertyOf <http://rdaregistry.info/Elements/w/P10047> ;
    skos:definition "Relates a work to a person, such as an advisor or supervisor of thesis or dissertation research, overseeing either an academic degree or thesis."@en .

<http://rdaregistry.info/Elements/w/P10042> a rdf:Property ;
    rdfs:label "has appellant person"@en ;
    rdakit:instructionNumber "18.5" ;
    rdakit:toolkitDefinition "A person who appeals a decision of a lower court recorded in a legal work of a higher court."@en,
        "Una persona que apela una decisión de una corte menor registrada en una obra jurídica de una corte superior."@es,
        "Personne qui en appelle de la décision d’un tribunal inférieur."@fr ;
    rdakit:toolkitLabel "appellant person"@en,
        "persona apelante"@es,
        "personne appelante"@fr ;
    reg:hasSubproperty <http://rdaregistry.info/Elements/w/object/P10042> ;
    reg:hasUnconstrained <http://rdaregistry.info/Elements/u/P60457> ;
    reg:lexicalAlias <http://rdaregistry.info/Elements/w/appellantPerson.en> ;
    reg:name "appellantPerson"@en ;
    reg:status <http://metadataregistry.org/uri/RegStatus/1001> ;
    rdfs:domain <http://rdaregistry.info/Elements/c/C10001> ;
    rdfs:isDefinedBy <http://rdaregistry.info/Elements/w/> ;
    rdfs:subPropertyOf <http://rdaregistry.info/Elements/w/P10038> ;
    skos:definition "Relates a work to a person who appeals a decision of a lower court recorded in a legal work of a higher court."@en .

<http://rdaregistry.info/Elements/w/P10043> a rdf:Property ;
    rdfs:label "has plaintiff person"@en ;
    rdakit:instructionNumber "18.5" ;
    rdakit:toolkitDefinition "A person who brings a suit in a civil proceeding."@en,
        "Una persona que presenta una demanda en un proceso civil."@es,
        "Personne qui intente une poursuite civile."@fr ;
    rdakit:toolkitLabel "plaintiff person"@en,
        "persona demandante"@es,
        "personne demanderesse"@fr ;
    reg:hasSubproperty <http://rdaregistry.info/Elements/w/object/P10043> ;
    reg:hasUnconstrained <http://rdaregistry.info/Elements/u/P60459> ;
    reg:lexicalAlias <http://rdaregistry.info/Elements/w/plaintiffPerson.en> ;
    reg:name "plaintiffPerson"@en ;
    reg:status <http://metadataregistry.org/uri/RegStatus/1001> ;
    rdfs:domain <http://rdaregistry.info/Elements/c/C10001> ;
    rdfs:isDefinedBy <http://rdaregistry.info/Elements/w/> ;
    rdfs:subPropertyOf <http://rdaregistry.info/Elements/w/P10039> ;
    skos:definition "Relates a work to a person who brings a suit in a civil proceeding."@en .

<http://rdaregistry.info/Elements/w/P10044> a rdf:Property ;
    rdfs:label "has judge"@en ;
    rdakit:instructionNumber "18.5" ;
    rdakit:toolkitDefinition "A person who hears and decides on legal matters in court."@en,
        "Una persona que escucha y se pronuncia sobre materias legales en un tribunal."@es,
        "Personne qui entend des causes juridiques et rend jugement dans un tribunal."@fr ;
    rdakit:toolkitLabel "judge"@en,
        "juez"@es,
        "juge"@fr ;
    reg:hasSubproperty <http://rdaregistry.info/Elements/w/object/P10044> ;
    reg:hasUnconstrained <http://rdaregistry.info/Elements/u/P60461> ;
    reg:lexicalAlias <http://rdaregistry.info/Elements/w/judge.en> ;
    reg:name "judge"@en ;
    reg:status <http://metadataregistry.org/uri/RegStatus/1001> ;
    rdfs:domain <http://rdaregistry.info/Elements/c/C10001> ;
    rdfs:isDefinedBy <http://rdaregistry.info/Elements/w/> ;
    rdfs:subPropertyOf <http://rdaregistry.info/Elements/w/P10047> ;
    skos:definition "Relates a work to a person who hears and decides on legal matters in court."@en .

<http://rdaregistry.info/Elements/w/P10045> a rdf:Property ;
    rdfs:label "has praeses"@en ;
    rdakit:instructionNumber "18.5" ;
    rdakit:toolkitDefinition "A person who is a faculty moderator of an academic disputation, normally proposing a thesis and participating in the ensuing disputation."@en,
        "Una persona del profesorado que actúa como árbitro de la facultad en un debate académico, normalmente proponiendo una tesis y participando en el debate consiguiente."@es,
        "Personne qui est le président d’une soutenance de thèse, proposant normalement la thèse et participant au débat qui s’ensuit."@fr ;
    rdakit:toolkitLabel "praeses"@en,
        "moderador académico"@es,
        "praeses"@fr ;
    reg:hasSubproperty <http://rdaregistry.info/Elements/w/object/P10045> ;
    reg:hasUnconstrained <http://rdaregistry.info/Elements/u/P60463> ;
    reg:lexicalAlias <http://rdaregistry.info/Elements/w/praeses.en> ;
    reg:name "praeses"@en ;
    reg:status <http://metadataregistry.org/uri/RegStatus/1001> ;
    rdfs:domain <http://rdaregistry.info/Elements/c/C10001> ;
    rdfs:isDefinedBy <http://rdaregistry.info/Elements/w/> ;
    rdfs:subPropertyOf <http://rdaregistry.info/Elements/w/P10065> ;
    skos:definition "Relates a work to a person who is a faculty moderator of an academic disputation, normally proposing a thesis and participating in the ensuing disputation."@en .

<http://rdaregistry.info/Elements/w/P10046> a rdf:Property ;
    rdfs:label "has issuing body"@en ;
    rdakit:instructionNumber "18.5" ;
    rdakit:toolkitDefinition "An agent issuing a work, such as an official organ of the body."@en,
        "Una persona, familia o entidad corporativa que publica una obra, tal como el órgano oficial de una entidad."@es,
        "Personne, famille ou collectivité publiant une œuvre, tel un organe officiel de l’organisme."@fr ;
    rdakit:toolkitLabel "issuing body"@en,
        "entidad editora"@es,
        "organisme de publication"@fr ;
    reg:hasSubproperty <http://rdaregistry.info/Elements/w/object/P10046> ;
    reg:hasUnconstrained <http://rdaregistry.info/Elements/u/P60467> ;
    reg:lexicalAlias <http://rdaregistry.info/Elements/w/issuingBody.en> ;
    reg:name "issuingBody"@en ;
    reg:status <http://metadataregistry.org/uri/RegStatus/1001> ;
    rdfs:domain <http://rdaregistry.info/Elements/c/C10001> ;
    rdfs:isDefinedBy <http://rdaregistry.info/Elements/w/> ;
    rdfs:subPropertyOf <http://rdaregistry.info/Elements/w/P10047> ;
    skos:definition "Relates a work to an agent issuing a work, such as an official organ of the body."@en .

<http://rdaregistry.info/Elements/w/P10048> a rdf:Property ;
    rdfs:label "has dedicator"@en ;
    rdakit:instructionNumber "18.5" ;
    rdakit:toolkitDefinition "An agent by whom a work is dedicated."@en,
        "Una persona, familia o entidad corporativa que dedica una obra."@es,
        "Personne, famille ou collectivité par qui une œuvre est dédiée."@fr ;
    rdakit:toolkitLabel "dedicator"@en,
        "autor de dedicación"@es,
        "dédicateur"@fr ;
    reg:hasSubproperty <http://rdaregistry.info/Elements/w/object/P10048> ;
    reg:hasUnconstrained <http://rdaregistry.info/Elements/u/P60375> ;
    reg:lexicalAlias <http://rdaregistry.info/Elements/w/dedicator.en> ;
    reg:name "dedicator"@en ;
    reg:status <http://metadataregistry.org/uri/RegStatus/1001> ;
    rdfs:domain <http://rdaregistry.info/Elements/c/C10001> ;
    rdfs:isDefinedBy <http://rdaregistry.info/Elements/w/> ;
    rdfs:subPropertyOf <http://rdaregistry.info/Elements/w/P10047> ;
    skos:definition "Relates a work to an agent by whom a work is dedicated."@en .

<http://rdaregistry.info/Elements/w/P10049> a rdf:Property ;
    rdfs:label "has honouree"@en ;
    rdakit:instructionNumber "18.5" ;
    rdakit:toolkitDefinition "An agent honoured by a work."@en,
        "Una persona, familia o entidad corporativa en cuyo honor se realiza una obra (por ej., quien es objeto de una obra conmemorativa)"@es,
        "Personne, famille ou collectivité honorée par une œuvre (par exemple, une personne à qui sont offerts des mélanges)."@fr ;
    rdakit:toolkitLabel "honouree"@en,
        "homenajeado"@es,
        "entité honorée"@fr ;
    reg:hasSubproperty <http://rdaregistry.info/Elements/w/object/P10049> ;
    reg:hasUnconstrained <http://rdaregistry.info/Elements/u/P60406> ;
    reg:lexicalAlias <http://rdaregistry.info/Elements/w/honouree.en> ;
    reg:name "honouree"@en ;
    reg:status <http://metadataregistry.org/uri/RegStatus/1001> ;
    rdfs:domain <http://rdaregistry.info/Elements/c/C10001> ;
    rdfs:isDefinedBy <http://rdaregistry.info/Elements/w/> ;
    rdfs:subPropertyOf <http://rdaregistry.info/Elements/w/P10047> ;
    skos:definition "Relates a work to an agent honoured by a work."@en .

<http://rdaregistry.info/Elements/w/P10050> a rdf:Property ;
    rdfs:label "has programmer"@en ;
    rdakit:instructionNumber "18.5" ;
    rdakit:toolkitDefinition "An agent responsible for creating a computer program."@en,
        "Una persona, familia o entidad corporativa responsable de la creación de un programa de computadora."@es,
        "Personne, famille ou collectivité responsable de la création d’un programme informatique."@fr ;
    rdakit:toolkitLabel "programmer"@en,
        "programador"@es,
        "programmeur"@fr ;
    reg:hasSubproperty <http://rdaregistry.info/Elements/w/object/P10050> ;
    reg:hasUnconstrained <http://rdaregistry.info/Elements/u/P60423> ;
    reg:lexicalAlias <http://rdaregistry.info/Elements/w/programmer.en> ;
    reg:name "programmer"@en ;
    reg:status <http://metadataregistry.org/uri/RegStatus/1001> ;
    rdfs:domain <http://rdaregistry.info/Elements/c/C10001> ;
    rdfs:isDefinedBy <http://rdaregistry.info/Elements/w/> ;
    rdfs:subPropertyOf <http://rdaregistry.info/Elements/w/P10065> ;
    skos:definition "Relates a work to an agent responsible for creating a computer program."@en .

<http://rdaregistry.info/Elements/w/P10051> a rdf:Property ;
    rdfs:label "has designer"@en ;
    rdakit:instructionNumber "18.5" ;
    rdakit:toolkitDefinition "An agent responsible for creating a design for an object."@en,
        "Una persona, familia o entidad corporativa responsable de la creación del diseño de un objeto."@es,
        "Personne, famille ou collectivité responsable de la conception d’un objet."@fr ;
    rdakit:toolkitLabel "designer"@en,
        "diseñador"@es,
        "designer"@fr ;
    reg:hasSubproperty <http://rdaregistry.info/Elements/w/object/P10051> ;
    reg:hasUnconstrained <http://rdaregistry.info/Elements/u/P60424> ;
    reg:lexicalAlias <http://rdaregistry.info/Elements/w/designer.en> ;
    reg:name "designer"@en ;
    reg:status <http://metadataregistry.org/uri/RegStatus/1001> ;
    rdfs:domain <http://rdaregistry.info/Elements/c/C10001> ;
    rdfs:isDefinedBy <http://rdaregistry.info/Elements/w/> ;
    rdfs:subPropertyOf <http://rdaregistry.info/Elements/w/P10065> ;
    skos:definition "Relates a work to an agent responsible for creating a design for an object."@en .

<http://rdaregistry.info/Elements/w/P10052> a rdf:Property ;
    rdfs:label "has cartographer"@en ;
    rdakit:instructionNumber "18.5" ;
    rdakit:toolkitDefinition "An agent responsible for creating a map, atlas, globe, or other cartographic work."@en,
        "Una persona, familia o entidad corporativa responsable de la creación de un mapa, atlas, globo u otra obra cartográfica."@es,
        "Personne, famille ou collectivité responsable de la création d’une carte, d’un atlas, d’un globe ou d’une autre œuvre cartographique."@fr ;
    rdakit:toolkitLabel "cartographer"@en,
        "cartógrafo"@es,
        "cartographe"@fr ;
    reg:hasSubproperty <http://rdaregistry.info/Elements/w/object/P10052> ;
    reg:hasUnconstrained <http://rdaregistry.info/Elements/u/P60425> ;
    reg:lexicalAlias <http://rdaregistry.info/Elements/w/cartographer.en> ;
    reg:name "cartographer"@en ;
    reg:status <http://metadataregistry.org/uri/RegStatus/1001> ;
    rdfs:domain <http://rdaregistry.info/Elements/c/C10001> ;
    rdfs:isDefinedBy <http://rdaregistry.info/Elements/w/> ;
    rdfs:subPropertyOf <http://rdaregistry.info/Elements/w/P10065> ;
    skos:definition "Relates a work to an agent responsible for creating a map, atlas, globe, or other cartographic work."@en .

<http://rdaregistry.info/Elements/w/P10053> a rdf:Property ;
    rdfs:label "has composer"@en ;
    rdakit:instructionNumber "18.5" ;
    rdakit:toolkitDefinition "An agent responsible for creating a musical work."@en,
        "Una persona, familia o entidad corporativa responsable de la creación de una obra musical."@es,
        "Personne, famille ou collectivité responsable de la création d’une œuvre musicale."@fr ;
    rdakit:toolkitLabel "composer"@en,
        "compositor"@es,
        "compositeur"@fr ;
    reg:hasSubproperty <http://rdaregistry.info/Elements/w/object/P10053> ;
    reg:hasUnconstrained <http://rdaregistry.info/Elements/u/P60426> ;
    reg:lexicalAlias <http://rdaregistry.info/Elements/w/composer.en> ;
    reg:name "composer"@en ;
    reg:status <http://metadataregistry.org/uri/RegStatus/1001> ;
    rdfs:domain <http://rdaregistry.info/Elements/c/C10001> ;
    rdfs:isDefinedBy <http://rdaregistry.info/Elements/w/> ;
    rdfs:subPropertyOf <http://rdaregistry.info/Elements/w/P10065> ;
    skos:definition "Relates a work to an agent responsible for creating a musical work."@en ;
    skos:scopeNote "Adaptation of another musical work to form a distinct alteration, paraphrasing a work or creating a work in the general style of another composer, or creating a work that is based on the music of another composer, is included."@en .

<http://rdaregistry.info/Elements/w/P10054> a rdf:Property ;
    rdfs:label "has inventor"@en ;
    rdakit:instructionNumber "18.5" ;
    rdakit:toolkitDefinition "An agent responsible for creating a new device or process."@en,
        "Una persona, familia o entidad corporativa responsable de la creación de un nuevo aparato o proceso."@es,
        "Personne, famille ou collectivité responsable de la création d’un nouveau dispositif ou procédé."@fr ;
    rdakit:toolkitLabel "inventor"@en,
        "inventor"@es,
        "inventeur"@fr ;
    reg:hasSubproperty <http://rdaregistry.info/Elements/w/object/P10054> ;
    reg:hasUnconstrained <http://rdaregistry.info/Elements/u/P60427> ;
    reg:lexicalAlias <http://rdaregistry.info/Elements/w/inventor.en> ;
    reg:name "inventor"@en ;
    reg:status <http://metadataregistry.org/uri/RegStatus/1001> ;
    rdfs:domain <http://rdaregistry.info/Elements/c/C10001> ;
    rdfs:isDefinedBy <http://rdaregistry.info/Elements/w/> ;
    rdfs:subPropertyOf <http://rdaregistry.info/Elements/w/P10065> ;
    skos:definition "Relates a work to an agent responsible for creating a new device or process."@en .

<http://rdaregistry.info/Elements/w/P10055> a rdf:Property ;
    rdfs:label "has compiler"@en ;
    rdakit:instructionNumber "18.5" ;
    rdakit:seeAlso <http://rdaregistry.info/Elements/e/P20048> ;
    rdakit:toolkitDefinition "An agent responsible for creating a new work such as a bibliography or a directory by selecting, arranging, aggregating, and editing data, information, etc."@en,
        "Una persona, familia o entidad corporativa responsable de la creación de una nueva obra (por ej., una bibliografía, un directorio) seleccionando, arreglando, agregando y editando datos, información, etc."@es,
        "Personne, famille ou collectivité responsable de la création d’une nouvelle œuvre (par exemple, une bibliographie, un répertoire) en sélectionnant, en organisant, en regroupant et en éditant des données, de l’information, etc."@fr ;
    rdakit:toolkitLabel "compiler"@en,
        "compilador"@es,
        "compilateur"@fr ;
    reg:hasSubproperty <http://rdaregistry.info/Elements/w/object/P10055> ;
    reg:hasUnconstrained <http://rdaregistry.info/Elements/u/P60428> ;
    reg:lexicalAlias <http://rdaregistry.info/Elements/w/compiler.en> ;
    reg:name "compiler"@en ;
    reg:status <http://metadataregistry.org/uri/RegStatus/1001> ;
    rdfs:domain <http://rdaregistry.info/Elements/c/C10001> ;
    rdfs:isDefinedBy <http://rdaregistry.info/Elements/w/> ;
    rdfs:subPropertyOf <http://rdaregistry.info/Elements/w/P10065> ;
    skos:definition "Relates a work to an agent responsible for creating a new work such as a bibliography or a directory by selecting, arranging, aggregating, and editing data, information, etc."@en ;
    skos:scopeNote "Revising or clarifying the content, or selecting and putting together works or parts of work, by one or more creators is excluded."@en .

<http://rdaregistry.info/Elements/w/P10056> a rdf:Property ;
    rdfs:label "has photographer"@en ;
    rdakit:instructionNumber "18.5" ;
    rdakit:toolkitDefinition "An agent responsible for creating a photographic work."@en,
        "Una personal, familia o entidad corporativa responsable de la creación de una obra fotográfica."@es,
        "Personne, famille ou collectivité responsable de la création d’une œuvre photographique."@fr ;
    rdakit:toolkitLabel "photographer"@en,
        "fotógrafo"@es,
        "photographe"@fr ;
    reg:hasSubproperty <http://rdaregistry.info/Elements/w/object/P10056> ;
    reg:hasUnconstrained <http://rdaregistry.info/Elements/u/P60429> ;
    reg:lexicalAlias <http://rdaregistry.info/Elements/w/photographer.en> ;
    reg:name "photographer"@en ;
    reg:status <http://metadataregistry.org/uri/RegStatus/1001> ;
    rdfs:domain <http://rdaregistry.info/Elements/c/C10001> ;
    rdfs:isDefinedBy <http://rdaregistry.info/Elements/w/> ;
    rdfs:subPropertyOf <http://rdaregistry.info/Elements/w/P10065> ;
    skos:definition "Relates a work to an agent responsible for creating a photographic work."@en .

<http://rdaregistry.info/Elements/w/P10057> a rdf:Property ;
    rdfs:label "has interviewer"@en ;
    rdakit:instructionNumber "18.5" ;
    rdakit:toolkitDefinition "An agent responsible for creating a work by acting as an interviewer, reporter, pollster, or some other information gathering agent."@en,
        "Una persona, familia o entidad corporativa responsable de la creación de una obra actuando como un entrevistador, un reportero u otro agente recolector de información."@es,
        "Personne, famille ou collectivité responsable de la création d’une œuvre en agissant à titre d’intervieweur, de journaliste, de sondeur ou d’autre agent recueillant de l’information."@fr ;
    rdakit:toolkitLabel "interviewer"@en,
        "entrevistador"@es,
        "intervieweur"@fr ;
    reg:hasSubproperty <http://rdaregistry.info/Elements/w/object/P10057> ;
    reg:hasUnconstrained <http://rdaregistry.info/Elements/u/P60430> ;
    reg:lexicalAlias <http://rdaregistry.info/Elements/w/interviewer.en> ;
    reg:name "interviewer"@en ;
    reg:status <http://metadataregistry.org/uri/RegStatus/1001> ;
    rdfs:domain <http://rdaregistry.info/Elements/c/C10001> ;
    rdfs:isDefinedBy <http://rdaregistry.info/Elements/w/> ;
    rdfs:subPropertyOf <http://rdaregistry.info/Elements/w/P10065> ;
    skos:definition "Relates a work to an agent responsible for creating a work by acting as an interviewer, reporter, pollster, or some other information gathering agent."@en .

<http://rdaregistry.info/Elements/w/P10059> a rdf:Property ;
    rdfs:label "has interviewee"@en ;
    rdakit:instructionNumber "18.5" ;
    rdakit:toolkitDefinition "An agent responsible for creating a work by responding to an interviewer, usually a reporter, pollster, or some other information gathering agent."@en,
        "Una persona, familia o entidad corporativa responsable de la creación de una obra mediante respuestas a un entrevistador, generalmente un reportero, encuestador u otro agente recolector de información."@es,
        "Personne, famille ou collectivité responsable de la création d’une œuvre en répondant à un intervieweur, habituellement un journaliste, un sondeur ou un autre agent recueillant de l’information."@fr ;
    rdakit:toolkitLabel "interviewee"@en,
        "entrevistado"@es,
        "interviewé"@fr ;
    reg:hasSubproperty <http://rdaregistry.info/Elements/w/object/P10059> ;
    reg:hasUnconstrained <http://rdaregistry.info/Elements/u/P60432> ;
    reg:lexicalAlias <http://rdaregistry.info/Elements/w/interviewee.en> ;
    reg:name "interviewee"@en ;
    reg:status <http://metadataregistry.org/uri/RegStatus/1001> ;
    rdfs:domain <http://rdaregistry.info/Elements/c/C10001> ;
    rdfs:isDefinedBy <http://rdaregistry.info/Elements/w/> ;
    rdfs:subPropertyOf <http://rdaregistry.info/Elements/w/P10065> ;
    skos:definition "Relates a work to an agent responsible for creating a work by responding to an interviewer, usually a reporter, pollster, or some other information gathering agent."@en .

<http://rdaregistry.info/Elements/w/P10060> a rdf:Property ;
    rdfs:label "has choreographer"@en ;
    rdakit:instructionNumber "18.5" ;
    rdakit:toolkitDefinition "An agent responsible for creating a work of movement."@en,
        "Una persona, familia o entidad corporativa responsable de la creación de una obra de movimiento."@es,
        "Personne, famille ou collectivité responsable de la création d’une œuvre de mouvement."@fr ;
    rdakit:toolkitLabel "choreographer"@en,
        "coreógrafo"@es,
        "chorégraphe"@fr ;
    reg:hasSubproperty <http://rdaregistry.info/Elements/w/object/P10060> ;
    reg:hasUnconstrained <http://rdaregistry.info/Elements/u/P60433> ;
    reg:lexicalAlias <http://rdaregistry.info/Elements/w/choreographer.en> ;
    reg:name "choreographer"@en ;
    reg:status <http://metadataregistry.org/uri/RegStatus/1001> ;
    rdfs:domain <http://rdaregistry.info/Elements/c/C10001> ;
    rdfs:isDefinedBy <http://rdaregistry.info/Elements/w/> ;
    rdfs:subPropertyOf <http://rdaregistry.info/Elements/w/P10065> ;
    skos:definition "Relates a work to an agent responsible for creating a work of movement."@en .

<http://rdaregistry.info/Elements/w/P10063> a rdf:Property ;
    rdfs:label "has filmmaker"@en ;
    rdakit:instructionNumber "18.5" ;
    rdakit:toolkitDefinition "An agent responsible for creating an independent or personal film."@en,
        "Una persona, familia o entidad corporativa responsable de la creación una película cinematográfica independiente o personal."@es,
        "Personne, famille ou collectivité responsable de la création d’un film indépendant ou personnel."@fr ;
    rdakit:toolkitLabel "filmmaker"@en,
        "cineasta"@es,
        "cinéaste"@fr ;
    reg:hasSubproperty <http://rdaregistry.info/Elements/w/object/P10063> ;
    reg:hasUnconstrained <http://rdaregistry.info/Elements/u/P60436> ;
    reg:lexicalAlias <http://rdaregistry.info/Elements/w/filmmaker.en> ;
    reg:name "filmmaker"@en ;
    reg:status <http://metadataregistry.org/uri/RegStatus/1001> ;
    rdfs:domain <http://rdaregistry.info/Elements/c/C10001> ;
    rdfs:isDefinedBy <http://rdaregistry.info/Elements/w/> ;
    rdfs:subPropertyOf <http://rdaregistry.info/Elements/w/P10065> ;
    skos:definition "Relates a work to an agent responsible for creating an independent or personal film."@en ;
    skos:scopeNote "A filmmaker is individually responsible for the conception and execution of all aspects of the film."@en .

<http://rdaregistry.info/Elements/w/P10067> a rdf:Property ;
    rdfs:label "has sponsoring body"@en ;
    rdakit:instructionNumber "18.5" ;
    rdakit:toolkitDefinition "An agent sponsoring some aspect of a work, such as funding research or sponsoring an event."@en,
        "Una persona, familia o entidad corporativa que patrocina algún aspecto de una obra, por ej., financiando una investigación, patrocinando un evento."@es,
        "Personne, famille ou collectivité commanditant certains aspects d’une œuvre, par exemple, le financement de la recherche, le parrainage d’un événement."@fr ;
    rdakit:toolkitLabel "sponsoring body"@en,
        "entidad patrocinadora"@es,
        "commanditaire"@fr ;
    reg:hasSubproperty <http://rdaregistry.info/Elements/w/object/P10067> ;
    reg:hasUnconstrained <http://rdaregistry.info/Elements/u/P60451> ;
    reg:lexicalAlias <http://rdaregistry.info/Elements/w/sponsoringBody.en> ;
    reg:name "sponsoringBody"@en ;
    reg:status <http://metadataregistry.org/uri/RegStatus/1001> ;
    rdfs:domain <http://rdaregistry.info/Elements/c/C10001> ;
    rdfs:isDefinedBy <http://rdaregistry.info/Elements/w/> ;
    rdfs:subPropertyOf <http://rdaregistry.info/Elements/w/P10047> ;
    skos:definition "Relates a work to an agent sponsoring some aspect of a work, such as funding research or sponsoring an event."@en .

<http://rdaregistry.info/Elements/w/P10068> a rdf:Property ;
    rdfs:label "has director of photography"@en ;
    rdakit:instructionNumber "18.5" ;
    rdakit:toolkitDefinition "An agent that captures images, either electronically or on film or video stock, and often selects and arranges the lighting."@en,
        "Una persona, familia o entidad corporativa que captura imágenes, ya sea almacenadas electrónicamente o en película o vídeo, y con frecuencia selecciona y arregla la iluminación."@es,
        "Personne, famille ou collectivité qui capte des images, de manière électronique ou bien sur film ou vidéo, et qui, souvent, choisit et dispose l’éclairage."@fr ;
    rdakit:toolkitLabel "director of photography"@en,
        "director de fotografía"@es,
        "directeur de la photographie"@fr ;
    reg:hasSubproperty <http://rdaregistry.info/Elements/w/object/P10068> ;
    reg:hasUnconstrained <http://rdaregistry.info/Elements/u/P60452> ;
    reg:lexicalAlias <http://rdaregistry.info/Elements/w/directorOfPhotography.en> ;
    reg:name "directorOfPhotography"@en ;
    reg:status <http://metadataregistry.org/uri/RegStatus/1001> ;
    rdfs:domain <http://rdaregistry.info/Elements/c/C10001> ;
    rdfs:isDefinedBy <http://rdaregistry.info/Elements/w/> ;
    rdfs:subPropertyOf <http://rdaregistry.info/Elements/w/P10047> ;
    skos:definition "Relates a work to an agent that captures images, either electronically or on film or video stock, and often selects and arranges the lighting."@en ;
    skos:scopeNote "The director of photography for a movie is also called the chief cinematographer."@en .

<http://rdaregistry.info/Elements/w/P10069> a rdf:Property ;
    rdfs:label "has dedicatee"@en ;
    rdakit:instructionNumber "18.5" ;
    rdakit:toolkitDefinition "An agent to whom a work is dedicated."@en,
        "Una persona, familia o entidad corporativa a la cual se dedicó una obra."@es,
        "Personne, famille ou collectivité à qui une œuvre est dédiée."@fr ;
    rdakit:toolkitLabel "dedicatee"@en,
        "destinatario de una dedicatoria"@es,
        "dédicataire"@fr ;
    reg:hasSubproperty <http://rdaregistry.info/Elements/w/object/P10069> ;
    reg:hasUnconstrained <http://rdaregistry.info/Elements/u/P60455> ;
    reg:lexicalAlias <http://rdaregistry.info/Elements/w/dedicatee.en> ;
    reg:name "dedicatee"@en ;
    reg:status <http://metadataregistry.org/uri/RegStatus/1001> ;
    rdfs:domain <http://rdaregistry.info/Elements/c/C10001> ;
    rdfs:isDefinedBy <http://rdaregistry.info/Elements/w/> ;
    rdfs:subPropertyOf <http://rdaregistry.info/Elements/w/P10047> ;
    skos:definition "Relates a work to an agent to whom a work is dedicated."@en .

<http://rdaregistry.info/Elements/w/P10070> a rdf:Property ;
    rdfs:label "has addressee"@en ;
    rdakit:instructionNumber "18.5" ;
    rdakit:toolkitDefinition "An agent to whom a work or part of a work is addressed."@en,
        "Una persona, familia o entidad corporativa a quien va dirigida una obra o parte de ella"@es,
        "Personne, famille ou collectivité à qui une œuvre ou une partie d’œuvre est adressée."@fr ;
    rdakit:toolkitLabel "addressee"@en,
        "destinatario"@es,
        "destinataire"@fr ;
    reg:hasSubproperty <http://rdaregistry.info/Elements/w/object/P10070> ;
    reg:hasUnconstrained <http://rdaregistry.info/Elements/u/P60456> ;
    reg:lexicalAlias <http://rdaregistry.info/Elements/w/addressee.en> ;
    reg:name "addressee"@en ;
    reg:status <http://metadataregistry.org/uri/RegStatus/1001> ;
    rdfs:domain <http://rdaregistry.info/Elements/c/C10001> ;
    rdfs:isDefinedBy <http://rdaregistry.info/Elements/w/> ;
    rdfs:subPropertyOf <http://rdaregistry.info/Elements/w/P10047> ;
    skos:definition "Relates a work to an agent to whom a work or part of a work is addressed."@en .

<http://rdaregistry.info/Elements/w/P10071> a rdf:Property ;
    rdfs:label "has consultant"@en ;
    rdakit:instructionNumber "18.5" ;
    rdakit:toolkitDefinition "An agent who provides consultation services, and often makes recommendations, for another agent that is represented as the creator of a work."@en,
        "Una persona, familia o entidad corporativa que proporciona servicios de consultoría, y que a menudo hace recomendaciones, a otra persona, familia o entidad corporativa que es representada como el creador de una obra."@es,
        "Personne, famille ou collectivité qui fournit des services de consultation et fait souvent des recommandations à une autre personne, famille ou collectivité représentée comme créatrice de l’œuvre."@fr ;
    rdakit:toolkitLabel "consultant"@en,
        "consultor"@es,
        "consultant"@fr ;
    reg:hasSubproperty <http://rdaregistry.info/Elements/w/object/P10071> ;
    reg:hasUnconstrained <http://rdaregistry.info/Elements/u/P60465> ;
    reg:lexicalAlias <http://rdaregistry.info/Elements/w/consultant.en> ;
    reg:name "consultant"@en ;
    reg:status <http://metadataregistry.org/uri/RegStatus/1001> ;
    rdfs:domain <http://rdaregistry.info/Elements/c/C10001> ;
    rdfs:isDefinedBy <http://rdaregistry.info/Elements/w/> ;
    rdfs:subPropertyOf <http://rdaregistry.info/Elements/w/P10047> ;
    skos:definition "Relates a work to an agent who provides consultation services, and often makes recommendations, for another agent that is represented as the creator of a work."@en .

<http://rdaregistry.info/Elements/w/P10073> a rdf:Property ;
    rdfs:label "has film producer"@en ;
    rdakit:instructionNumber "18.5" ;
    rdakit:toolkitDefinition "A producer responsible for most of the business aspects of a film."@en,
        "Un productor responsable de la mayor parte de los aspectos empresariales relacionados con una película cinematográfica."@es,
        "Producteur responsable de la majeure partie des aspects financiers, techniques et artistiques d’un film."@fr ;
    rdakit:toolkitLabel "film producer"@en,
        "productor cinematográfico"@es,
        "producteur de films"@fr ;
    reg:hasSubproperty <http://rdaregistry.info/Elements/w/object/P10073> ;
    reg:hasUnconstrained <http://rdaregistry.info/Elements/u/P60169> ;
    reg:lexicalAlias <http://rdaregistry.info/Elements/w/filmProducer.en> ;
    reg:name "filmProducer"@en ;
    reg:status <http://metadataregistry.org/uri/RegStatus/1001> ;
    rdfs:domain <http://rdaregistry.info/Elements/c/C10001> ;
    rdfs:isDefinedBy <http://rdaregistry.info/Elements/w/> ;
    rdfs:subPropertyOf <http://rdaregistry.info/Elements/w/P10064> ;
    skos:definition "Relates a work to a producer responsible for most of the business aspects of a film."@en .

<http://rdaregistry.info/Elements/w/P10074> a rdf:Property ;
    rdfs:label "has radio producer"@en ;
    rdakit:instructionNumber "18.5" ;
    rdakit:toolkitDefinition "A producer responsible for most of the business aspects of a radio program."@en,
        "Un productor responsable de la mayor parte de los aspectos empresariales relacionados con un programa de radio."@es,
        "Producteur responsable de la majeure partie des aspects financiers, techniques et artistiques d’une émission de radio."@fr ;
    rdakit:toolkitLabel "radio producer"@en,
        "productor de radio"@es,
        "producteur d’émissions de radio"@fr ;
    reg:hasSubproperty <http://rdaregistry.info/Elements/w/object/P10074> ;
    reg:hasUnconstrained <http://rdaregistry.info/Elements/u/P60170> ;
    reg:lexicalAlias <http://rdaregistry.info/Elements/w/radioProducer.en> ;
    reg:name "radioProducer"@en ;
    reg:status <http://metadataregistry.org/uri/RegStatus/1001> ;
    rdfs:domain <http://rdaregistry.info/Elements/c/C10001> ;
    rdfs:isDefinedBy <http://rdaregistry.info/Elements/w/> ;
    rdfs:subPropertyOf <http://rdaregistry.info/Elements/w/P10064> ;
    skos:definition "Relates a work to a producer responsible for most of the business aspects of a radio program."@en .

<http://rdaregistry.info/Elements/w/P10075> a rdf:Property ;
    rdfs:label "has television producer"@en ;
    rdakit:instructionNumber "18.5" ;
    rdakit:toolkitDefinition "A producer responsible for most of the business aspects of a television program."@en,
        "Un productor responsable de la mayor parte de los aspectos empresariales relacionados con un programa de televisión."@es,
        "Producteur responsable de la majeure partie des aspects financiers, techniques et artistiques d’une émission de télévision."@fr ;
    rdakit:toolkitLabel "television producer"@en,
        "productor de televisión"@es,
        "producteur d’émissions de télévision"@fr ;
    reg:hasSubproperty <http://rdaregistry.info/Elements/w/object/P10075> ;
    reg:hasUnconstrained <http://rdaregistry.info/Elements/u/P60171> ;
    reg:lexicalAlias <http://rdaregistry.info/Elements/w/televisionProducer.en> ;
    reg:name "televisionProducer"@en ;
    reg:status <http://metadataregistry.org/uri/RegStatus/1001> ;
    rdfs:domain <http://rdaregistry.info/Elements/c/C10001> ;
    rdfs:isDefinedBy <http://rdaregistry.info/Elements/w/> ;
    rdfs:subPropertyOf <http://rdaregistry.info/Elements/w/P10064> ;
    skos:definition "Relates a work to a producer responsible for most of the business aspects of a television program."@en .

<http://rdaregistry.info/Elements/w/P10076> a rdf:Property ;
    rdfs:label "is adapted as radio program (work)"@en ;
    rdakit:instructionNumber "24.5" ;
    rdakit:toolkitDefinition "A radio program based on a source work."@en,
        "Un programa de radio basado en la obra fuente."@es,
        "Émission de radio basée sur l’œuvre source."@fr ;
    rdakit:toolkitLabel "adapted as radio program (work)"@en,
        "adaptada como programa de radio (obra)"@es,
        "adapté en émission de radio (œuvre)"@fr ;
    reg:hasSubproperty <http://rdaregistry.info/Elements/w/object/P10076> ;
    reg:hasUnconstrained <http://rdaregistry.info/Elements/u/P60174> ;
    reg:lexicalAlias <http://rdaregistry.info/Elements/w/adaptedAsRadioProgramWork.en> ;
    reg:name "adaptedAsRadioProgramWork"@en ;
    reg:status <http://metadataregistry.org/uri/RegStatus/1001> ;
    rdfs:domain <http://rdaregistry.info/Elements/c/C10001> ;
    rdfs:isDefinedBy <http://rdaregistry.info/Elements/w/> ;
    rdfs:subPropertyOf <http://rdaregistry.info/Elements/w/P10155> ;
    skos:definition "Relates a work to a radio program based on a source work."@en .

<http://rdaregistry.info/Elements/w/P10080> a rdf:Property ;
    rdfs:label "is subseries"@en ;
    rdakit:instructionNumber "24.5" ;
    rdakit:toolkitDefinition "A serial or multipart work that consistently appears in a larger work; a title of a larger work appears on all issues or parts of a subseries."@en,
        "Una serie u obra en varias partes que aparece constantemente en conjunto con otra serie generalmente más amplia; el título de la obra más amplia aparece en todos los números o partes de la subserie."@es,
        "Publication en série ou œuvre en plusieurs parties qui apparaît régulièrement dans une œuvre plus vaste ; le titre de l’œuvre plus vaste apparaît sur toutes les livraisons ou parties de la sous-collection."@fr ;
    rdakit:toolkitLabel "subseries"@en,
        "subserie"@es,
        "sous-collection"@fr ;
    reg:hasSubproperty <http://rdaregistry.info/Elements/w/object/P10080> ;
    reg:hasUnconstrained <http://rdaregistry.info/Elements/u/P60316> ;
    reg:lexicalAlias <http://rdaregistry.info/Elements/w/subseries.en> ;
    reg:name "subseries"@en ;
    reg:status <http://metadataregistry.org/uri/RegStatus/1001> ;
    rdfs:domain <http://rdaregistry.info/Elements/c/C10001> ;
    rdfs:isDefinedBy <http://rdaregistry.info/Elements/w/> ;
    rdfs:subPropertyOf <http://rdaregistry.info/Elements/w/P10147> ;
    skos:definition "Relates a work to a serial or multipart work that consistently appears in a larger work; a title of a larger work appears on all issues or parts of a subseries"@en .

<http://rdaregistry.info/Elements/w/P10081> a rdf:Property ;
    rdfs:label "has longitude and latitude"@en,
        "har longitud och latitud"@sv ;
    rdakit:instructionNumber "7.4.2" ;
    rdakit:toolkitDefinition "A system for identifying the area covered by the cartographic content of a work using longitude of the westernmost and easternmost boundaries and latitude of the northernmost and southernmost boundaries."@en,
        "Un sistema para identificar el área cubierta por el contenido cartográfico de un recurso."@es,
        "Système permettant d’identifier la surface couverte par le contenu cartographique d’une ressource en utilisant la longitude des limites ouest et est et la latitude des limites nord et sud."@fr ;
    rdakit:toolkitLabel "longitude and latitude"@en,
        "longitud y latitud"@es,
        "longitude et latitude"@fr,
        "longitud och latitud"@sv ;
    reg:hasSubproperty <http://rdaregistry.info/Elements/w/P10300>,
        <http://rdaregistry.info/Elements/w/P10301> ;
    reg:hasUnconstrained <http://rdaregistry.info/Elements/u/P60345> ;
    reg:lexicalAlias <http://rdaregistry.info/Elements/w/longitudeAndLatitude.en> ;
    reg:name "longitudeAndLatitude"@en ;
    reg:status <http://metadataregistry.org/uri/RegStatus/1001> ;
    rdfs:domain <http://rdaregistry.info/Elements/c/C10001> ;
    rdfs:isDefinedBy <http://rdaregistry.info/Elements/w/> ;
    rdfs:subPropertyOf <http://rdaregistry.info/Elements/w/P10024> ;
    skos:definition "Relates a work to a system for identifying the area covered by the cartographic content of a work using longitude of the westernmost and easternmost boundaries and latitude of the northernmost and southernmost boundaries."@en .

<http://rdaregistry.info/Elements/w/P10082> a rdf:Property ;
    rdfs:label "has right ascension and declination"@en,
        "har rektascension och deklination"@sv ;
    rdakit:instructionNumber "7.4.4" ;
    rdakit:toolkitDefinition "A system for identifying the location of a celestial object in the sky covered by the cartographic content of a work using the angles of right ascension and declination."@en,
        "Un sistema para identificar la localización de un objeto celeste en el firmamento que está incluido en el contenido cartográfico de un recurso que utiliza los ángulos de ascensión directa y de declinación."@es,
        "Système utilisant les angles d’ascension droite et de déclinaison pour identifier la localisation d’un objet céleste dans la zone du ciel couverte par le contenu cartographique d’une ressource."@fr ;
    rdakit:toolkitLabel "right ascension and declination"@en,
        "ascensión recta y declinación"@es,
        "ascension droite et déclinaison"@fr,
        "rektascension och deklination"@sv ;
    reg:hasSubproperty <http://rdaregistry.info/Elements/w/P10302>,
        <http://rdaregistry.info/Elements/w/P10303> ;
    reg:hasUnconstrained <http://rdaregistry.info/Elements/u/P60346> ;
    reg:lexicalAlias <http://rdaregistry.info/Elements/w/rightAscensionAndDeclination.en> ;
    reg:name "rightAscensionAndDeclination"@en ;
    reg:status <http://metadataregistry.org/uri/RegStatus/1001> ;
    rdfs:domain <http://rdaregistry.info/Elements/c/C10001> ;
    rdfs:isDefinedBy <http://rdaregistry.info/Elements/w/> ;
    rdfs:subPropertyOf <http://rdaregistry.info/Elements/w/P10024> ;
    skos:definition "Relates a work to a system for identifying the location of a celestial object in the sky covered by the cartographic content of a work using the angles of right ascension and declination."@en .

<http://rdaregistry.info/Elements/w/P10083> a rdf:Property ;
    rdfs:label "has strings of coordinate pairs"@en ;
    rdakit:instructionNumber "7.4.3" ;
    rdakit:toolkitDefinition "A system for identifying the precise area covered by the cartographic content of a work using coordinates for each vertex of a polygon."@en,
        "Un sistema para identificar el área precisa incluida en el contenido cartográfico de un recurso utilizando coordenadas para cada vértice de un polígono."@es,
        "Système pour identifier la zone précise couverte par le contenu cartographique d’une ressource en utilisant des coordonnées pour chaque sommet d’un polygone."@fr ;
    rdakit:toolkitLabel "strings of coordinate pairs"@en,
        "cadenas de pares de coordenadas"@es,
        "chaînes de paires de coordonnées"@fr ;
    reg:hasUnconstrained <http://rdaregistry.info/Elements/u/P60347> ;
    reg:lexicalAlias <http://rdaregistry.info/Elements/w/stringsOfCoordinatePairs.en> ;
    reg:name "stringsOfCoordinatePairs"@en ;
    reg:status <http://metadataregistry.org/uri/RegStatus/1001> ;
    rdfs:domain <http://rdaregistry.info/Elements/c/C10001> ;
    rdfs:isDefinedBy <http://rdaregistry.info/Elements/w/> ;
    rdfs:subPropertyOf <http://rdaregistry.info/Elements/w/P10024> ;
    skos:definition "Relates a work to a system for identifying the precise area covered by the cartographic content of a work using coordinates for each vertex of a polygon."@en .

<http://rdaregistry.info/Elements/w/P10085> a rdf:Property ;
    rdfs:label "is adapted as television program (work)"@en ;
    rdakit:instructionNumber "24.5" ;
    rdakit:toolkitDefinition "A television program based on a source work."@en,
        "Un programa de televisión basado en la obra fuente"@es,
        "Émission de télévision basée sur l’œuvre source."@fr ;
    rdakit:toolkitLabel "adapted as television program (work)"@en,
        "adaptada como programa para televisión (obra)"@es,
        "adapté en émission de télévision (œuvre)"@fr ;
    reg:hasSubproperty <http://rdaregistry.info/Elements/w/object/P10085> ;
    reg:hasUnconstrained <http://rdaregistry.info/Elements/u/P60354> ;
    reg:lexicalAlias <http://rdaregistry.info/Elements/w/adaptedAsTelevisionProgramWork.en> ;
    reg:name "adaptedAsTelevisionProgramWork"@en ;
    reg:status <http://metadataregistry.org/uri/RegStatus/1001> ;
    rdfs:domain <http://rdaregistry.info/Elements/c/C10001> ;
    rdfs:isDefinedBy <http://rdaregistry.info/Elements/w/> ;
    rdfs:subPropertyOf <http://rdaregistry.info/Elements/w/P10155> ;
    skos:definition "Relates a work to a television program based on a source work."@en .

<http://rdaregistry.info/Elements/w/P10086> a rdf:Property ;
    rdfs:label "has variant title for work"@en,
        "har varianttitel för verket"@sv ;
    rdakit:instructionNumber "6.2.3" ;
    rdakit:toolkitDefinition "A title or form of title by which a work is known that differs from a title or form of title chosen as a preferred title for the work."@en,
        "Un título o una forma del título, por la que se conoce una obra que difiere del título o de la forma del título elegida como el título preferido de la obra."@es,
        "Titre ou forme de titre sous laquelle une œuvre est connue et qui diffère du titre ou de la forme de titre choisie comme titre privilégié de l’œuvre."@fr ;
    rdakit:toolkitLabel "variant title for work"@en,
        "variante de título de una obra"@es,
        "variante de titre de l’œuvre"@fr,
        "varianttitel för verket"@sv ;
    reg:hasUnconstrained <http://rdaregistry.info/Elements/u/P60355> ;
    reg:lexicalAlias <http://rdaregistry.info/Elements/w/variantTitleForWork.en> ;
    reg:name "variantTitleForWork"@en ;
    reg:status <http://metadataregistry.org/uri/RegStatus/1001> ;
    rdfs:domain <http://rdaregistry.info/Elements/c/C10001> ;
    rdfs:isDefinedBy <http://rdaregistry.info/Elements/w/> ;
    rdfs:subPropertyOf <http://rdaregistry.info/Elements/w/P10088> ;
    skos:definition "Relates a work to a title or form of title by which a work is known that differs from a title or form of title chosen as a preferred title for the work."@en ;
    skos:scopeNote "Variant title for work includes a title or form of title appearing on a manifestation of the work or found in reference sources, a title resulting from a different transliteration of a title, etc."@en .

<http://rdaregistry.info/Elements/w/P10087> a rdf:Property ;
    rdfs:label "is adapted as video (work)"@en ;
    rdakit:instructionNumber "24.5" ;
    rdakit:toolkitDefinition "A video based on a source work."@en,
        "Un video basado en la obra fuente."@es,
        "Vidéo basée sur l’œuvre source."@fr ;
    rdakit:toolkitLabel "adapted as video (work)"@en,
        "adaptada como video (obra)"@es,
        "adapté en vidéo (œuvre)"@fr ;
    reg:hasSubproperty <http://rdaregistry.info/Elements/w/object/P10087> ;
    reg:hasUnconstrained <http://rdaregistry.info/Elements/u/P60361> ;
    reg:lexicalAlias <http://rdaregistry.info/Elements/w/adaptedAsVideoWork.en> ;
    reg:name "adaptedAsVideoWork"@en ;
    reg:status <http://metadataregistry.org/uri/RegStatus/1001> ;
    rdfs:domain <http://rdaregistry.info/Elements/c/C10001> ;
    rdfs:isDefinedBy <http://rdaregistry.info/Elements/w/> ;
    rdfs:subPropertyOf <http://rdaregistry.info/Elements/w/P10155> ;
    skos:definition "Relates a work to a video based on a source work."@en .

<http://rdaregistry.info/Elements/w/P10089> a rdf:Property ;
    rdfs:label "is abstracted in (work)"@en ;
    rdakit:instructionNumber "24.5" ;
    rdakit:toolkitDefinition "A work that is an abstracting and indexing service that abstracts the contents of a source work."@en,
        "Una obra (un servicio de indización y resúmenes) que resume el contenido de una entidad fuente."@es,
        "Œuvre (service d’analyse et d’indexation) qui résume le contenu d’une œuvre source."@fr ;
    rdakit:toolkitLabel "abstracted in (work)"@en,
        "resumida en (obra)"@es,
        "résumé analytiquement dans (œuvre)"@fr ;
    reg:hasSubproperty <http://rdaregistry.info/Elements/w/object/P10089> ;
    reg:hasUnconstrained <http://rdaregistry.info/Elements/u/P60177> ;
    reg:lexicalAlias <http://rdaregistry.info/Elements/w/abstractedInWork.en> ;
    reg:name "abstractedInWork"@en ;
    reg:status <http://metadataregistry.org/uri/RegStatus/1001> ;
    rdfs:domain <http://rdaregistry.info/Elements/c/C10001> ;
    rdfs:isDefinedBy <http://rdaregistry.info/Elements/w/> ;
    rdfs:subPropertyOf <http://rdaregistry.info/Elements/w/P10148> ;
    skos:definition "Relates a work to a work that is an abstracting and indexing service that abstracts the contents of a source work."@en .

<http://rdaregistry.info/Elements/w/P10090> a rdf:Property ;
    rdfs:label "is indexed in (work)"@en ;
    rdakit:instructionNumber "24.5" ;
    rdakit:toolkitDefinition "A work that is an abstracting and indexing service that indexes the contents of a source work."@en,
        "Una obra (un servicio de indización y resúmenes) que indiza el contenido de la obra fuente."@es,
        "Œuvre (service d’analyse et d’indexation) qui indexe le contenu de l’œuvre source."@fr ;
    rdakit:toolkitLabel "indexed in (work)"@en,
        "indizada en (obra)"@es,
        "indexé dans (œuvre)"@fr ;
    reg:hasSubproperty <http://rdaregistry.info/Elements/w/object/P10090> ;
    reg:hasUnconstrained <http://rdaregistry.info/Elements/u/P60178> ;
    reg:lexicalAlias <http://rdaregistry.info/Elements/w/indexedInWork.en> ;
    reg:name "indexedInWork"@en ;
    reg:status <http://metadataregistry.org/uri/RegStatus/1001> ;
    rdfs:domain <http://rdaregistry.info/Elements/c/C10001> ;
    rdfs:isDefinedBy <http://rdaregistry.info/Elements/w/> ;
    rdfs:subPropertyOf <http://rdaregistry.info/Elements/w/P10148> ;
    skos:definition "Relates a work to a work that is an abstracting and indexing service that indexes the contents of a source work."@en .

<http://rdaregistry.info/Elements/w/P10091> a rdf:Property ;
    rdfs:label "is adapted as choreography (work)"@en ;
    rdakit:instructionNumber "24.5" ;
    rdakit:toolkitDefinition "A work consisting of movement based on a source work."@en,
        "Una obra que consiste en movimiento (p. ej., danza) basada en la obra fuente."@es,
        "Œuvre consistant en mouvement (par exemple, de la danse) basée sur l’œuvre source."@fr ;
    rdakit:toolkitLabel "adapted as choreography (work)"@en,
        "adaptada como coreografía (obra)"@es,
        "adapté en chorégraphie (œuvre)"@fr ;
    reg:hasSubproperty <http://rdaregistry.info/Elements/w/object/P10091> ;
    reg:hasUnconstrained <http://rdaregistry.info/Elements/u/P60180> ;
    reg:lexicalAlias <http://rdaregistry.info/Elements/w/adaptedAsChoreographyWork.en> ;
    reg:name "adaptedAsChoreographyWork"@en ;
    reg:status <http://metadataregistry.org/uri/RegStatus/1001> ;
    rdfs:domain <http://rdaregistry.info/Elements/c/C10001> ;
    rdfs:isDefinedBy <http://rdaregistry.info/Elements/w/> ;
    rdfs:subPropertyOf <http://rdaregistry.info/Elements/w/P10155> ;
    skos:definition "Relates a work to a work consisting of movement based on a source work."@en .

<http://rdaregistry.info/Elements/w/P10092> a rdf:Property ;
    rdfs:label "is errata (work)"@en ;
    rdakit:instructionNumber "24.5" ;
    rdakit:toolkitDefinition "A work consisting of errors discovered after the publication of a predominant work, with their corrections."@en,
        "Una obra que consiste en errores descubiertos después de la publicación de la obra principal, con sus correcciones."@es,
        "Œuvre constituée des erreurs découvertes après la publication de l’œuvre prédominante, avec leurs corrections."@fr ;
    rdakit:toolkitLabel "errata (work)"@en,
        "fe de erratas (obra)"@es,
        "errata (œuvre)"@fr ;
    reg:hasSubproperty <http://rdaregistry.info/Elements/w/object/P10092> ;
    reg:hasUnconstrained <http://rdaregistry.info/Elements/u/P60181> ;
    reg:lexicalAlias <http://rdaregistry.info/Elements/w/errataWork.en> ;
    reg:name "errataWork"@en ;
    reg:status <http://metadataregistry.org/uri/RegStatus/1001> ;
    rdfs:domain <http://rdaregistry.info/Elements/c/C10001> ;
    rdfs:isDefinedBy <http://rdaregistry.info/Elements/w/> ;
    rdfs:subPropertyOf <http://rdaregistry.info/Elements/w/P10108> ;
    skos:definition "Relates a work to a work consisting of errors discovered after the publication of a predominant work, with their corrections."@en .

<http://rdaregistry.info/Elements/w/P10093> a rdf:Property ;
    rdfs:label "is illustrations (work)"@en ;
    rdakit:instructionNumber "24.5" ;
    rdakit:toolkitDefinition "A work consisting of pictorial content designed to explain or decorate an augmented work."@en,
        "Una obra que consiste en contenido pictórico diseñado para explicar o decorar la obra aumentada."@es,
        "Œuvre consistant en contenu visuel destiné à expliquer ou à décorer l’œuvre augmentée."@fr ;
    rdakit:toolkitLabel "illustrations (work)"@en,
        "ilustraciones (obra)"@es,
        "illustrations (œuvre)"@fr ;
    reg:hasSubproperty <http://rdaregistry.info/Elements/w/object/P10093> ;
    reg:hasUnconstrained <http://rdaregistry.info/Elements/u/P60182> ;
    reg:lexicalAlias <http://rdaregistry.info/Elements/w/illustrationsWork.en> ;
    reg:name "illustrationsWork"@en ;
    reg:status <http://metadataregistry.org/uri/RegStatus/1001> ;
    rdfs:domain <http://rdaregistry.info/Elements/c/C10001> ;
    rdfs:isDefinedBy <http://rdaregistry.info/Elements/w/> ;
    rdfs:subPropertyOf <http://rdaregistry.info/Elements/w/P10108> ;
    skos:definition "Relates a work to a work consisting of pictorial content designed to explain or decorate an augmented work."@en .

<http://rdaregistry.info/Elements/w/P10094> a rdf:Property ;
    rdfs:label "is adapted as motion picture screenplay (work)"@en ;
    rdakit:instructionNumber "24.5" ;
    rdakit:toolkitDefinition "A work consisting of a screenplay for a motion picture, based on a source work."@en,
        "Una obra que consiste en un guión para una película cinematográfica, basado en la obra fuente."@es,
        "Œuvre consistant en le scénario pour un film, basée sur l’œuvre source."@fr ;
    rdakit:toolkitLabel "adapted as motion picture screenplay (work)"@en,
        "adaptada como guión cinematográfico (obra)"@es,
        "adapté en scénario de film (œuvre)"@fr ;
    reg:hasSubproperty <http://rdaregistry.info/Elements/w/object/P10094> ;
    reg:hasUnconstrained <http://rdaregistry.info/Elements/u/P60184> ;
    reg:lexicalAlias <http://rdaregistry.info/Elements/w/adaptedAsMotionPictureScreenplayWork.en> ;
    reg:name "adaptedAsMotionPictureScreenplayWork"@en ;
    reg:status <http://metadataregistry.org/uri/RegStatus/1001> ;
    rdfs:domain <http://rdaregistry.info/Elements/c/C10001> ;
    rdfs:isDefinedBy <http://rdaregistry.info/Elements/w/> ;
    rdfs:subPropertyOf <http://rdaregistry.info/Elements/w/P10095> ;
    skos:definition "Relates a work to a work consisting of a screenplay for a motion picture, based on a source work."@en .

<http://rdaregistry.info/Elements/w/P10096> a rdf:Property ;
    rdfs:label "is adapted as television screenplay (work)"@en ;
    rdakit:instructionNumber "24.5" ;
    rdakit:toolkitDefinition "A work consisting of a screenplay for a television program, based on a source work."@en,
        "Una obra que consiste en un guión para un programa de televisión, basado en la obra fuente."@es,
        "Œuvre consistant en le scénario pour une émission de télévision, basée sur l’œuvre source."@fr ;
    rdakit:toolkitLabel "adapted as television screenplay (work)"@en,
        "adaptada como guión para televisión (obra)"@es,
        "adapté en scénario de télévision (œuvre)"@fr ;
    reg:hasSubproperty <http://rdaregistry.info/Elements/w/object/P10096> ;
    reg:hasUnconstrained <http://rdaregistry.info/Elements/u/P60186> ;
    reg:lexicalAlias <http://rdaregistry.info/Elements/w/adaptedAsTelevisionScreenplayWork.en> ;
    reg:name "adaptedAsTelevisionScreenplayWork"@en ;
    reg:status <http://metadataregistry.org/uri/RegStatus/1001> ;
    rdfs:domain <http://rdaregistry.info/Elements/c/C10001> ;
    rdfs:isDefinedBy <http://rdaregistry.info/Elements/w/> ;
    rdfs:subPropertyOf <http://rdaregistry.info/Elements/w/P10095> ;
    skos:definition "Relates a work to a work consisting of a screenplay for a television program, based on a source work."@en .

<http://rdaregistry.info/Elements/w/P10097> a rdf:Property ;
    rdfs:label "is adapted as video screenplay (work)"@en ;
    rdakit:instructionNumber "24.5" ;
    rdakit:toolkitDefinition "A work consisting of a screenplay for a video, based on a source work."@en,
        "Una obra que consiste en un guión para video, basado en la obra fuente."@es,
        "Œuvre consistant en le scénario pour une vidéo, basée sur l’œuvre source."@fr ;
    rdakit:toolkitLabel "adapted as video screenplay (work)"@en,
        "adaptada como guión para video (obra)"@es,
        "adapté en scénario de vidéo (œuvre)"@fr ;
    reg:hasSubproperty <http://rdaregistry.info/Elements/w/object/P10097> ;
    reg:hasUnconstrained <http://rdaregistry.info/Elements/u/P60187> ;
    reg:lexicalAlias <http://rdaregistry.info/Elements/w/adaptedAsVideoScreenplayWork.en> ;
    reg:name "adaptedAsVideoScreenplayWork"@en ;
    reg:status <http://metadataregistry.org/uri/RegStatus/1001> ;
    rdfs:domain <http://rdaregistry.info/Elements/c/C10001> ;
    rdfs:isDefinedBy <http://rdaregistry.info/Elements/w/> ;
    rdfs:subPropertyOf <http://rdaregistry.info/Elements/w/P10095> ;
    skos:definition "Relates a work to a work consisting of a screenplay for a video, based on a source work."@en .

<http://rdaregistry.info/Elements/w/P10098> a rdf:Property ;
    rdfs:label "is adapted as radio script (work)"@en ;
    rdakit:instructionNumber "24.5" ;
    rdakit:toolkitDefinition "A work consisting of a script for a radio program, based on a source work."@en,
        "Una obra que consiste en el guión para un programa de radio, basado en la obra fuente."@es,
        "Œuvre consistant en le script d’une émission de radio, basée sur l’œuvre source."@fr ;
    rdakit:toolkitLabel "adapted as radio script (work)"@en,
        "adaptada como guión radiofónico (obra)"@es,
        "adapté en script radiophonique (œuvre)"@fr ;
    reg:hasSubproperty <http://rdaregistry.info/Elements/w/object/P10098> ;
    reg:hasUnconstrained <http://rdaregistry.info/Elements/u/P60188> ;
    reg:lexicalAlias <http://rdaregistry.info/Elements/w/adaptedAsRadioScriptWork.en> ;
    reg:name "adaptedAsRadioScriptWork"@en ;
    reg:status <http://metadataregistry.org/uri/RegStatus/1001> ;
    rdfs:domain <http://rdaregistry.info/Elements/c/C10001> ;
    rdfs:isDefinedBy <http://rdaregistry.info/Elements/w/> ;
    rdfs:subPropertyOf <http://rdaregistry.info/Elements/w/P10155> ;
    skos:definition "Relates a work to a work consisting of a script for a radio program, based on a source work."@en .

<http://rdaregistry.info/Elements/w/P10099> a rdf:Property ;
    rdfs:label "is freely translated as (work)"@en ;
    rdakit:instructionNumber "24.5" ;
    rdakit:toolkitDefinition "A work that is both an adaptation and a translation into another language of a source work."@en,
        "Una obra creada mediante la interpretación libre de la obra fuente en otra lengua, preservando el espíritu del original, pero no sus detalles lingüísticos"@es,
        "Œuvre créée en traduisant librement l’œuvre source dans une autre langue, de façon à préserver l’esprit de l’original, mais non ses particularités linguistiques."@fr ;
    rdakit:toolkitLabel "freely translated as (work)"@en,
        "traducida libremente como (obra)"@es,
        "librement traduit comme (œuvre)"@fr ;
    reg:hasSubproperty <http://rdaregistry.info/Elements/w/object/P10099> ;
    reg:hasUnconstrained <http://rdaregistry.info/Elements/u/P60189> ;
    reg:lexicalAlias <http://rdaregistry.info/Elements/w/freelyTranslatedAsWork.en> ;
    reg:name "freelyTranslatedAsWork"@en ;
    reg:status <http://metadataregistry.org/uri/RegStatus/1001> ;
    rdfs:domain <http://rdaregistry.info/Elements/c/C10001> ;
    rdfs:isDefinedBy <http://rdaregistry.info/Elements/w/> ;
    rdfs:subPropertyOf <http://rdaregistry.info/Elements/w/P10148> ;
    skos:definition "Relates a work to a work that is both an adaptation and a translation into another language of a source work."@en .

<http://rdaregistry.info/Elements/w/P10101> a rdf:Property ;
    rdfs:label "is subseries of"@en ;
    rdakit:instructionNumber "24.5" ;
    rdakit:toolkitDefinition "A work in which a part consistently appears; a title of a larger work appears on all issues or parts of a subseries."@en,
        "Una obra en la que la parte aparece en forma consistente; el título de la obra mayor aparece en todas las entregas o partes de la subserie."@es,
        "Œuvre dans laquelle la partie apparaît régulièrement ; le titre de l’œuvre plus vaste apparaît sur toutes les livraisons ou parties de la sous-collection."@fr ;
    rdakit:toolkitLabel "subseries of"@en,
        "subserie de (obra)"@es,
        "sous-collection de"@fr ;
    reg:hasSubproperty <http://rdaregistry.info/Elements/w/object/P10101> ;
    reg:hasUnconstrained <http://rdaregistry.info/Elements/u/P60192> ;
    reg:lexicalAlias <http://rdaregistry.info/Elements/w/subseriesOf.en> ;
    reg:name "subseriesOf"@en ;
    reg:status <http://metadataregistry.org/uri/RegStatus/1001> ;
    rdfs:domain <http://rdaregistry.info/Elements/c/C10001> ;
    rdfs:isDefinedBy <http://rdaregistry.info/Elements/w/> ;
    rdfs:subPropertyOf <http://rdaregistry.info/Elements/w/P10019> ;
    skos:definition "Relates a work to a work in which a part consistently appears; a title of a larger work appears on all issues or parts of a subseries."@en .

<http://rdaregistry.info/Elements/w/P10102> a rdf:Property ;
    rdfs:label "is in series"@en ;
    rdakit:instructionNumber "24.5" ;
    rdakit:toolkitDefinition "A work in which a part has been issued; a title of a larger work appears on the part."@en,
        "Una obra en la cual se publica la parte; el título de la obra mayor aparece en la parte."@es,
        "Œuvre dans laquelle la partie a été publiée ; le titre de l’œuvre plus vaste apparaît sur la partie."@fr ;
    rdakit:toolkitLabel "in series"@en,
        "en la serie (obra)"@es,
        "dans la collection"@fr ;
    reg:hasSubproperty <http://rdaregistry.info/Elements/w/object/P10102> ;
    reg:hasUnconstrained <http://rdaregistry.info/Elements/u/P60193> ;
    reg:lexicalAlias <http://rdaregistry.info/Elements/w/inSeries.en> ;
    reg:name "inSeries"@en ;
    reg:status <http://metadataregistry.org/uri/RegStatus/1001> ;
    rdfs:domain <http://rdaregistry.info/Elements/c/C10001> ;
    rdfs:isDefinedBy <http://rdaregistry.info/Elements/w/> ;
    rdfs:subPropertyOf <http://rdaregistry.info/Elements/w/P10019> ;
    skos:definition "Relates a work to a work in which a part has been issued; a title of the larger work appears on the part."@en .

<http://rdaregistry.info/Elements/w/P10104> a rdf:Property ;
    rdfs:label "is continued in part by (work)"@en ;
    rdakit:instructionNumber "24.5" ;
    rdakit:toolkitDefinition "A work part of whose content separated from an earlier work to form a new work."@en,
        "Una obra de la cual parte de su contenido se separa de una obra anterior para formar una nueva obra."@es,
        "Œuvre dont une partie du contenu a été détachée d’une œuvre antérieure pour former une nouvelle œuvre."@fr ;
    rdakit:toolkitLabel "continued in part by (work)"@en,
        "continuada en parte por (obra)"@es,
        "continué en partie par (œuvre)"@fr ;
    reg:hasSubproperty <http://rdaregistry.info/Elements/w/object/P10104> ;
    reg:hasUnconstrained <http://rdaregistry.info/Elements/u/P60199> ;
    reg:lexicalAlias <http://rdaregistry.info/Elements/w/continuedInPartByWork.en> ;
    reg:name "continuedInPartByWork"@en ;
    reg:status <http://metadataregistry.org/uri/RegStatus/1001> ;
    rdfs:domain <http://rdaregistry.info/Elements/c/C10001> ;
    rdfs:isDefinedBy <http://rdaregistry.info/Elements/w/> ;
    rdfs:subPropertyOf <http://rdaregistry.info/Elements/w/P10170> ;
    skos:definition "Relates a work to a work part of whose content separated from an earlier work to form a new work."@en ;
    skos:scopeNote "This relationship applies generally to serials."@en .

<http://rdaregistry.info/Elements/w/P10106> a rdf:Property ;
    rdfs:label "is incidental music for (work)"@en ;
    rdakit:instructionNumber "24.5" ;
    rdakit:toolkitDefinition "A work such as a play or other spoken work for the stage that uses a musical work as incidental music."@en,
        "Una obra tal como una obra de teatro u otra obra hablada para escenario que utiliza la obra musica como música incidental."@es,
        "Œuvre telle qu’une pièce de théâtre ou une autre œuvre parlée pour la scène qui utilise l’œuvre musicale comme musique de scène."@fr ;
    rdakit:toolkitLabel "incidental music for (work)"@en,
        "música incidental para (obra)"@es,
        "musique de scène pour (œuvre)"@fr ;
    reg:hasSubproperty <http://rdaregistry.info/Elements/w/object/P10106> ;
    reg:hasUnconstrained <http://rdaregistry.info/Elements/u/P60202> ;
    reg:lexicalAlias <http://rdaregistry.info/Elements/w/incidentalMusicForWork.en> ;
    reg:name "incidentalMusicForWork"@en ;
    reg:status <http://metadataregistry.org/uri/RegStatus/1001> ;
    rdfs:domain <http://rdaregistry.info/Elements/c/C10001> ;
    rdfs:isDefinedBy <http://rdaregistry.info/Elements/w/> ;
    rdfs:subPropertyOf <http://rdaregistry.info/Elements/w/P10238> ;
    skos:definition "Relates a work to a work such as a play or other spoken work for the stage that uses a musical work as incidental music."@en .

<http://rdaregistry.info/Elements/w/P10107> a rdf:Property ;
    rdfs:label "is abstracted as (work)"@en ;
    rdakit:instructionNumber "24.5" ;
    rdakit:toolkitDefinition "A work that abbreviates a source work in a brief, objective manner."@en,
        "Una obra que abrevia la obra fuente en una manera breve y objetiva."@es,
        "Œuvre qui abrège l’œuvre source d’une manière brève et objective."@fr ;
    rdakit:toolkitLabel "abstracted as (work)"@en,
        "resumida como (obra)"@es,
        "résumé analytiquement comme (œuvre)"@fr ;
    reg:hasSubproperty <http://rdaregistry.info/Elements/w/object/P10107> ;
    reg:hasUnconstrained <http://rdaregistry.info/Elements/u/P60203> ;
    reg:lexicalAlias <http://rdaregistry.info/Elements/w/abstractedAsWork.en> ;
    reg:name "abstractedAsWork"@en ;
    reg:status <http://metadataregistry.org/uri/RegStatus/1001> ;
    rdfs:domain <http://rdaregistry.info/Elements/c/C10001> ;
    rdfs:isDefinedBy <http://rdaregistry.info/Elements/w/> ;
    rdfs:subPropertyOf <http://rdaregistry.info/Elements/w/P10148> ;
    skos:definition "Relates a work to a work that abbreviates a source work in a brief, objective manner."@en .

<http://rdaregistry.info/Elements/w/P10109> a rdf:Property ;
    rdfs:label "is summarized as (work)"@en ;
    rdakit:instructionNumber "24.5" ;
    rdakit:toolkitDefinition "A work that consists of a brief recapitulation of the content of a source work."@en,
        "Una obra que contiene una recapitulación breve del contenido de la obra fuente."@es,
        "Œuvre qui consiste en une brève récapitulation du contenu de l’œuvre source."@fr ;
    rdakit:toolkitLabel "summarized as (work)"@en,
        "sumarizada como (obra)"@es,
        "résumé comme (œuvre)"@fr ;
    reg:hasSubproperty <http://rdaregistry.info/Elements/w/object/P10109> ;
    reg:hasUnconstrained <http://rdaregistry.info/Elements/u/P60205> ;
    reg:lexicalAlias <http://rdaregistry.info/Elements/w/summarizedAsWork.en> ;
    reg:name "summarizedAsWork"@en ;
    reg:status <http://metadataregistry.org/uri/RegStatus/1001> ;
    rdfs:domain <http://rdaregistry.info/Elements/c/C10001> ;
    rdfs:isDefinedBy <http://rdaregistry.info/Elements/w/> ;
    rdfs:subPropertyOf <http://rdaregistry.info/Elements/w/P10148> ;
    skos:definition "Relates a work to a work that consists of a brief recapitulation of the content of a source work."@en .

<http://rdaregistry.info/Elements/w/P10110> a rdf:Property ;
    rdfs:label "is catalogue (work)"@en ;
    rdakit:instructionNumber "24.5" ;
    rdakit:toolkitDefinition "A work that consists of a complete enumeration of items arranged systematically."@en,
        "Una obra que contiene una enumeración completa de ítems ordenados sistemáticamente."@es,
        "Œuvre qui consiste en une énumération complète des items classés systématiquement."@fr ;
    rdakit:toolkitLabel "catalogue (work)"@en,
        "catálogo (obra)"@es,
        "catalogue (œuvre)"@fr ;
    reg:hasSubproperty <http://rdaregistry.info/Elements/w/object/P10110> ;
    reg:hasUnconstrained <http://rdaregistry.info/Elements/u/P60206> ;
    reg:lexicalAlias <http://rdaregistry.info/Elements/w/catalogueWork.en> ;
    reg:name "catalogueWork"@en ;
    reg:status <http://metadataregistry.org/uri/RegStatus/1001> ;
    rdfs:domain <http://rdaregistry.info/Elements/c/C10001> ;
    rdfs:isDefinedBy <http://rdaregistry.info/Elements/w/> ;
    rdfs:subPropertyOf <http://rdaregistry.info/Elements/w/P10108> ;
    skos:definition "Relates a work to a work that consists of a complete enumeration of items arranged systematically."@en .

<http://rdaregistry.info/Elements/w/P10111> a rdf:Property ;
    rdfs:label "is concordance (work)"@en ;
    rdakit:instructionNumber "24.5" ;
    rdakit:toolkitDefinition "A work that consists of an index of all the words in a predominant work."@en,
        "Una obra que consiste en un indice de todas las palabras en la obra principal."@es,
        "Œuvre qui consiste en un index de tous les mots de l’œuvre prédominante."@fr ;
    rdakit:toolkitLabel "concordance (work)"@en,
        "concordancia (obra)"@es,
        "concordance (œuvre)"@fr ;
    reg:hasSubproperty <http://rdaregistry.info/Elements/w/object/P10111> ;
    reg:hasUnconstrained <http://rdaregistry.info/Elements/u/P60208> ;
    reg:lexicalAlias <http://rdaregistry.info/Elements/w/concordanceWork.en> ;
    reg:name "concordanceWork"@en ;
    reg:status <http://metadataregistry.org/uri/RegStatus/1001> ;
    rdfs:domain <http://rdaregistry.info/Elements/c/C10001> ;
    rdfs:isDefinedBy <http://rdaregistry.info/Elements/w/> ;
    rdfs:subPropertyOf <http://rdaregistry.info/Elements/w/P10108> ;
    skos:definition "Relates a work to a work that consists of an index of all the words in a predominant work."@en .

<http://rdaregistry.info/Elements/w/P10112> a rdf:Property ;
    rdfs:label "is addenda (work)"@en ;
    rdakit:instructionNumber "24.5" ;
    rdakit:toolkitDefinition "A work consisting of brief content that is essential for the completeness of another work."@en,
        "Una obra que consiste en un material adicional breve, menos extenso que un suplemento, pero que es esencial para la integridad del texto de la obra principal; generalmente se agrega al final del contenido, pero que también puede publicarse en forma separada."@es,
        "Œuvre qui consiste en brèves informations additionnelles, moins étendues qu’un supplément, mais essentielles à la complétude du texte de l’œuvre prédominante ; ces informations sont généralement ajoutées à la fin du contenu, mais peuvent aussi parfois être publiées séparément."@fr ;
    rdakit:toolkitLabel "addenda (work)"@en,
        "adenda (obra)"@es,
        "addenda (œuvre)"@fr ;
    reg:hasSubproperty <http://rdaregistry.info/Elements/w/object/P10112> ;
    reg:hasUnconstrained <http://rdaregistry.info/Elements/u/P60209> ;
    reg:lexicalAlias <http://rdaregistry.info/Elements/w/addendaWork.en> ;
    reg:name "addendaWork"@en ;
    reg:status <http://metadataregistry.org/uri/RegStatus/1001> ;
    rdfs:domain <http://rdaregistry.info/Elements/c/C10001> ;
    rdfs:isDefinedBy <http://rdaregistry.info/Elements/w/> ;
    rdfs:subPropertyOf <http://rdaregistry.info/Elements/w/P10108> ;
    skos:definition "Relates a work to a work consisting of brief content that is essential for the completeness of another work."@en .

<http://rdaregistry.info/Elements/w/P10113> a rdf:Property ;
    rdfs:label "is adapted as libretto (work)"@en ;
    rdakit:instructionNumber "24.5" ;
    rdakit:toolkitDefinition "A work consisting of the text of an opera or other work for the musical stage, or an oratorio, based on a source work."@en,
        "Una obra que consiste en un texto de una ópera para representación musical o un oratorio, basada en la obra fuente."@es,
        "Œuvre qui consiste en le texte d’un opéra ou d’une autre œuvre pour la scène musicale, ou bien d’un oratorio, basée sur l’œuvre source."@fr ;
    rdakit:toolkitLabel "adapted as libretto (work)"@en,
        "adaptada como libreto (obra)"@es,
        "adapté en livret (œuvre)"@fr ;
    reg:hasSubproperty <http://rdaregistry.info/Elements/w/object/P10113> ;
    reg:hasUnconstrained <http://rdaregistry.info/Elements/u/P60210> ;
    reg:lexicalAlias <http://rdaregistry.info/Elements/w/adaptedAsLibrettoWork.en> ;
    reg:name "adaptedAsLibrettoWork"@en ;
    reg:status <http://metadataregistry.org/uri/RegStatus/1001> ;
    rdfs:domain <http://rdaregistry.info/Elements/c/C10001> ;
    rdfs:isDefinedBy <http://rdaregistry.info/Elements/w/> ;
    rdfs:subPropertyOf <http://rdaregistry.info/Elements/w/P10155> ;
    skos:definition "Relates a work to a work consisting of the text of an opera or other work for the musical stage, or an oratorio, based on a source work."@en .

<http://rdaregistry.info/Elements/w/P10114> a rdf:Property ;
    rdfs:label "is reviewed in (work)"@en ;
    rdakit:instructionNumber "23.5" ;
    rdakit:toolkitDefinition "A work that contains a brief evaluation of a described work."@en,
        "Una obra que contiene una evaluación breve de la obra descrita."@es,
        "Œuvre qui contient une brève évaluation de l’œuvre décrite."@fr ;
    rdakit:toolkitLabel "reviewed in (work)"@en,
        "reseñada en (obra)"@es,
        "recensé dans (œuvre)"@fr ;
    reg:hasSubproperty <http://rdaregistry.info/Elements/w/object/P10114> ;
    reg:hasUnconstrained <http://rdaregistry.info/Elements/u/P60211> ;
    reg:lexicalAlias <http://rdaregistry.info/Elements/w/reviewedInWork.en> ;
    reg:name "reviewedInWork"@en ;
    reg:status <http://metadataregistry.org/uri/RegStatus/1001> ;
    rdfs:domain <http://rdaregistry.info/Elements/c/C10001> ;
    rdfs:isDefinedBy <http://rdaregistry.info/Elements/w/> ;
    rdfs:subPropertyOf <http://rdaregistry.info/Elements/w/P10118> ;
    skos:definition "Relates a work to a work that contains a brief evaluation of a described work."@en .

<http://rdaregistry.info/Elements/w/P10115> a rdf:Property ;
    rdfs:label "is critiqued in (work)"@en ;
    rdakit:instructionNumber "23.5" ;
    rdakit:toolkitDefinition "A work that contains a critical evaluation of a described work."@en,
        "Una obra que contiene una evaluación crítica de la obra descrita."@es,
        "Œuvre qui contient une évaluation critique de l’œuvre décrite."@fr ;
    rdakit:toolkitLabel "critiqued in (work)"@en,
        "criticada en (obra)"@es,
        "critiqué dans (œuvre)"@fr ;
    reg:hasSubproperty <http://rdaregistry.info/Elements/w/object/P10115> ;
    reg:hasUnconstrained <http://rdaregistry.info/Elements/u/P60212> ;
    reg:lexicalAlias <http://rdaregistry.info/Elements/w/critiquedInWork.en> ;
    reg:name "critiquedInWork"@en ;
    reg:status <http://metadataregistry.org/uri/RegStatus/1001> ;
    rdfs:domain <http://rdaregistry.info/Elements/c/C10001> ;
    rdfs:isDefinedBy <http://rdaregistry.info/Elements/w/> ;
    rdfs:subPropertyOf <http://rdaregistry.info/Elements/w/P10118> ;
    skos:definition "Relates a work to a work that contains a critical evaluation of a described work."@en .

<http://rdaregistry.info/Elements/w/P10116> a rdf:Property ;
    rdfs:label "is commentary in (work)"@en ;
    rdakit:instructionNumber "23.5" ;
    rdakit:toolkitDefinition "A work that contains a set of explanatory or critical notes on a described work"@en,
        "Una obra que contiene un conjunto de notas explicativas o críticas sobre la obra descrita."@es,
        "Œuvre qui contient un ensemble de notes explicatives ou critiques sur l’œuvre décrite."@fr ;
    rdakit:toolkitLabel "commentary in (work)"@en,
        "comentario en (obra)"@es,
        "commentaire dans (œuvre)"@fr ;
    reg:hasSubproperty <http://rdaregistry.info/Elements/w/object/P10116> ;
    reg:hasUnconstrained <http://rdaregistry.info/Elements/u/P60213> ;
    reg:lexicalAlias <http://rdaregistry.info/Elements/w/commentaryInWork.en> ;
    reg:name "commentaryInWork"@en ;
    reg:status <http://metadataregistry.org/uri/RegStatus/1001> ;
    rdfs:domain <http://rdaregistry.info/Elements/c/C10001> ;
    rdfs:isDefinedBy <http://rdaregistry.info/Elements/w/> ;
    rdfs:subPropertyOf <http://rdaregistry.info/Elements/w/P10118> ;
    skos:definition "Relates a work to a work that contains a set of explanatory or critical notes on a described work."@en .

<http://rdaregistry.info/Elements/w/P10119> a rdf:Property ;
    rdfs:label "is expanded as (work)"@en ;
    rdakit:instructionNumber "24.5" ;
    rdakit:toolkitDefinition "A work that enlarges upon the content of a source work."@en,
        "Una obra que extiende el contenido de la obra fuente."@es,
        "Œuvre qui accroît le contenu de l’œuvre source."@fr ;
    rdakit:toolkitLabel "expanded as (work)"@en,
        "ampliada como (obra)"@es,
        "augmenté comme (œuvre)"@fr ;
    reg:hasSubproperty <http://rdaregistry.info/Elements/w/object/P10119> ;
    reg:hasUnconstrained <http://rdaregistry.info/Elements/u/P60216> ;
    reg:lexicalAlias <http://rdaregistry.info/Elements/w/expandedAsWork.en> ;
    reg:name "expandedAsWork"@en ;
    reg:status <http://metadataregistry.org/uri/RegStatus/1001> ;
    rdfs:domain <http://rdaregistry.info/Elements/c/C10001> ;
    rdfs:isDefinedBy <http://rdaregistry.info/Elements/w/> ;
    rdfs:subPropertyOf <http://rdaregistry.info/Elements/w/P10148> ;
    skos:definition "Relates a work to a work that enlarges upon the content of a source work."@en .

<http://rdaregistry.info/Elements/w/P10120> a rdf:Property ;
    rdfs:label "is evaluated in (work)"@en ;
    rdakit:instructionNumber "23.5" ;
    rdakit:toolkitDefinition "A work that examines or judges a described work."@en,
        "Una obra que examina o juzga la obra descrita."@es,
        "Œuvre qui examine ou juge l’œuvre décrite."@fr ;
    rdakit:toolkitLabel "evaluated in (work)"@en,
        "evaluada en (obra)"@es,
        "évalué dans (œuvre)"@fr ;
    reg:hasSubproperty <http://rdaregistry.info/Elements/w/object/P10120> ;
    reg:hasUnconstrained <http://rdaregistry.info/Elements/u/P60218> ;
    reg:lexicalAlias <http://rdaregistry.info/Elements/w/evaluatedInWork.en> ;
    reg:name "evaluatedInWork"@en ;
    reg:status <http://metadataregistry.org/uri/RegStatus/1001> ;
    rdfs:domain <http://rdaregistry.info/Elements/c/C10001> ;
    rdfs:isDefinedBy <http://rdaregistry.info/Elements/w/> ;
    rdfs:subPropertyOf <http://rdaregistry.info/Elements/w/P10118> ;
    skos:definition "Relates a work to a work that examines or judges a described work."@en .

<http://rdaregistry.info/Elements/w/P10121> a rdf:Property ;
    rdfs:label "is analysed in (work)"@en ;
    rdakit:instructionNumber "23.5" ;
    rdakit:toolkitDefinition "A work that examines a source work to identify its components and their relations."@en,
        "Una obra que examina la obra fuente para identificar sus componentes y sus relaciones."@es,
        "Œuvre qui examine l’œuvre source pour identifier ses composantes et leurs relations."@fr ;
    rdakit:toolkitLabel "analysed in (work)"@en,
        "analizada en (obra)"@es,
        "analysé dans (œuvre)"@fr ;
    reg:hasSubproperty <http://rdaregistry.info/Elements/w/object/P10121> ;
    reg:hasUnconstrained <http://rdaregistry.info/Elements/u/P60219> ;
    reg:lexicalAlias <http://rdaregistry.info/Elements/w/analysedInWork.en> ;
    reg:name "analysedInWork"@en ;
    reg:status <http://metadataregistry.org/uri/RegStatus/1001> ;
    rdfs:domain <http://rdaregistry.info/Elements/c/C10001> ;
    rdfs:isDefinedBy <http://rdaregistry.info/Elements/w/> ;
    rdfs:subPropertyOf <http://rdaregistry.info/Elements/w/P10118> ;
    skos:definition "Relates a work to a work that examines a source work to identify its components and their relations."@en .

<http://rdaregistry.info/Elements/w/P10122> a rdf:Property ;
    rdfs:label "is prequel"@en ;
    rdakit:instructionNumber "24.5" ;
    rdakit:toolkitDefinition "A work that extends the narrative of an earlier work backwards in time."@en,
        "Una obra que extiende la narración de una obra anterior hacia atrás en el tiempo."@es,
        "Œuvre qui étend le récit d’une œuvre antérieure sur une période plus ancienne dans le temps."@fr ;
    rdakit:toolkitLabel "prequel"@en,
        "precuela"@es,
        "antépisode"@fr ;
    reg:hasSubproperty <http://rdaregistry.info/Elements/w/object/P10122> ;
    reg:hasUnconstrained <http://rdaregistry.info/Elements/u/P60220> ;
    reg:lexicalAlias <http://rdaregistry.info/Elements/w/prequel.en> ;
    reg:name "prequel"@en ;
    reg:status <http://metadataregistry.org/uri/RegStatus/1001> ;
    rdfs:domain <http://rdaregistry.info/Elements/c/C10001> ;
    rdfs:isDefinedBy <http://rdaregistry.info/Elements/w/> ;
    rdfs:subPropertyOf <http://rdaregistry.info/Elements/w/P10156> ;
    skos:definition "Relates a work to a work that extends the narrative of an earlier work backwards in time."@en .

<http://rdaregistry.info/Elements/w/P10123> a rdf:Property ;
    rdfs:label "is appendix (work)"@en ;
    rdakit:instructionNumber "24.5" ;
    rdakit:toolkitDefinition "A work whose content augments another work."@en,
        "Una obra que constituye una ampliación de otra obra y que no es esencial para la integridad del contenido, como una lista de referencias, tablas estadísticas, un tema explicativo; puede ser material que va al final del contenido de la obra principal, o que puede publicarse en forma separada."@es,
        "Œuvre qui forme une partie augmentante d’une autre œuvre et qui n’est pas essentielle à la complétude du contenu, telle qu’une liste de références, des tableaux statistiques et des indications explicatives ; elle peut soit figurer à la fin du contenu de l’œuvre prédominante, soit être publiée séparément."@fr ;
    rdakit:toolkitLabel "appendix (work)"@en,
        "apéndice (obra)"@es,
        "annexe (œuvre)"@fr ;
    reg:hasSubproperty <http://rdaregistry.info/Elements/w/object/P10123> ;
    reg:hasUnconstrained <http://rdaregistry.info/Elements/u/P60221> ;
    reg:lexicalAlias <http://rdaregistry.info/Elements/w/appendixWork.en> ;
    reg:name "appendixWork"@en ;
    reg:status <http://metadataregistry.org/uri/RegStatus/1001> ;
    rdfs:domain <http://rdaregistry.info/Elements/c/C10001> ;
    rdfs:isDefinedBy <http://rdaregistry.info/Elements/w/> ;
    rdfs:subPropertyOf <http://rdaregistry.info/Elements/w/P10108> ;
    skos:definition "Relates a work to a work whose content augments another work."@en ;
    skos:scopeNote "Includes lists of references, statistical tables, and explanatory matter that are not essential to the completeness of the content."@en .

<http://rdaregistry.info/Elements/w/P10124> a rdf:Property ;
    rdfs:label "is guide (work)"@en ;
    rdakit:instructionNumber "24.5" ;
    rdakit:toolkitDefinition "A work that guides a user through the use of a predominant work, using notes, learning and study aids, exercises, problems, questions and answers, instructor or student materials, etc."@en,
        "Una obra que guía al usuario en el uso de la obra principal, utilizando notas, ayudas de aprendizaje y estudio, ejercicios, problemas, preguntas y respuestas, materiales para el instructor o el estudiante, etc."@es,
        "Œuvre qui guide un utilisateur à travers l’œuvre prédominante au moyen de notes, d’outils pédagogiques, d’exercices, de problèmes, de questions et réponses, de matériel didactique, etc."@fr ;
    rdakit:toolkitLabel "guide (work)"@en,
        "guía (obra)"@es,
        "guide (œuvre)"@fr ;
    reg:hasSubproperty <http://rdaregistry.info/Elements/w/object/P10124> ;
    reg:hasUnconstrained <http://rdaregistry.info/Elements/u/P60222> ;
    reg:lexicalAlias <http://rdaregistry.info/Elements/w/guideWork.en> ;
    reg:name "guideWork"@en ;
    reg:status <http://metadataregistry.org/uri/RegStatus/1001> ;
    rdfs:domain <http://rdaregistry.info/Elements/c/C10001> ;
    rdfs:isDefinedBy <http://rdaregistry.info/Elements/w/> ;
    rdfs:subPropertyOf <http://rdaregistry.info/Elements/w/P10108> ;
    skos:definition "Relates a work to a work that guides a user through the use of a predominant work, using notes, learning and study aids, exercises, problems, questions and answers, instructor or student materials, etc."@en .

<http://rdaregistry.info/Elements/w/P10125> a rdf:Property ;
    rdfs:label "is abridgement of (work)"@en ;
    rdakit:instructionNumber "24.5" ;
    rdakit:toolkitDefinition "A work that has been abridged, i.e., shortened without changing the general meaning or manner of presentation of a source work."@en,
        "Una obra que ha sido abreviada, i.e., acortada sin cambiar el significado general o manera de presentación de la obra fuente."@es,
        "Œuvre qui a été abrégée, c’est-à-dire raccourcie sans changer le sens général ou le mode de présentation de l’œuvre source."@fr ;
    rdakit:toolkitLabel "abridgement of (work)"@en,
        "abreviada de (obra)"@es,
        "abrégé de (œuvre)"@fr ;
    reg:hasSubproperty <http://rdaregistry.info/Elements/w/object/P10125> ;
    reg:hasUnconstrained <http://rdaregistry.info/Elements/u/P60223> ;
    reg:lexicalAlias <http://rdaregistry.info/Elements/w/abridgementOfWork.en> ;
    reg:name "abridgementOfWork"@en ;
    reg:status <http://metadataregistry.org/uri/RegStatus/1001> ;
    rdfs:domain <http://rdaregistry.info/Elements/c/C10001> ;
    rdfs:isDefinedBy <http://rdaregistry.info/Elements/w/> ;
    rdfs:subPropertyOf <http://rdaregistry.info/Elements/w/P10190> ;
    skos:definition "Relates a work to a work that has been abridged, i.e., shortened without changing the general meaning or manner of presentation of a source work."@en .

<http://rdaregistry.info/Elements/w/P10126> a rdf:Property ;
    rdfs:label "is abstract of (work)"@en ;
    rdakit:instructionNumber "24.5" ;
    rdakit:toolkitDefinition "A work that has been abstracted, i.e., abbreviated in a brief, objective manner."@en,
        "Una obra que ha sido resumida, i.e., abreviada en una forma breve y objetiva."@es,
        "Œuvre qui a été résumée analytiquement, c’est-à-dire abrégée d’une manière brève et objective."@fr ;
    rdakit:toolkitLabel "abstract of (work)"@en,
        "resumen de (obra)"@es,
        "résumé analytique de (œuvre)"@fr ;
    reg:hasSubproperty <http://rdaregistry.info/Elements/w/object/P10126> ;
    reg:hasUnconstrained <http://rdaregistry.info/Elements/u/P60224> ;
    reg:lexicalAlias <http://rdaregistry.info/Elements/w/abstractOfWork.en> ;
    reg:name "abstractOfWork"@en ;
    reg:status <http://metadataregistry.org/uri/RegStatus/1001> ;
    rdfs:domain <http://rdaregistry.info/Elements/c/C10001> ;
    rdfs:isDefinedBy <http://rdaregistry.info/Elements/w/> ;
    rdfs:subPropertyOf <http://rdaregistry.info/Elements/w/P10190> ;
    skos:definition "Relates a work to a work that has been abstracted, i.e., abbreviated in a brief, objective manner."@en .

<http://rdaregistry.info/Elements/w/P10127> a rdf:Property ;
    rdfs:label "is dramatization of (work)"@en ;
    rdakit:instructionNumber "24.5" ;
    rdakit:toolkitDefinition "A work that has been adapted as a drama."@en,
        "Una obra que ha sido adaptada como drama."@es,
        "Œuvre qui a été adaptée en pièce de théâtre."@fr ;
    rdakit:toolkitLabel "dramatization of (work)"@en,
        "dramatización de (obra)"@es,
        "adaptation au théâtre de (œuvre)"@fr ;
    reg:hasSubproperty <http://rdaregistry.info/Elements/w/object/P10127> ;
    reg:hasUnconstrained <http://rdaregistry.info/Elements/u/P60225> ;
    reg:lexicalAlias <http://rdaregistry.info/Elements/w/dramatizationOfWork.en> ;
    reg:name "dramatizationOfWork"@en ;
    reg:status <http://metadataregistry.org/uri/RegStatus/1001> ;
    rdfs:domain <http://rdaregistry.info/Elements/c/C10001> ;
    rdfs:isDefinedBy <http://rdaregistry.info/Elements/w/> ;
    rdfs:subPropertyOf <http://rdaregistry.info/Elements/w/P10142> ;
    skos:definition "Relates a work to a work that has been adapted as a drama."@en .

<http://rdaregistry.info/Elements/w/P10128> a rdf:Property ;
    rdfs:label "is verse adaptation of (work)"@en ;
    rdakit:instructionNumber "24.5" ;
    rdakit:toolkitDefinition "A work that has been adapted as a literary composition in verse form."@en,
        "Una obra que ha sido adaptada como una composición literaria en forma de verso."@es,
        "Œuvre qui a été adaptée sous forme de composition littéraire en vers."@fr ;
    rdakit:toolkitLabel "verse adaptation of (work)"@en,
        "adaptación en verso de (obra)"@es,
        "adaptation en vers de (œuvre)"@fr ;
    reg:hasSubproperty <http://rdaregistry.info/Elements/w/object/P10128> ;
    reg:hasUnconstrained <http://rdaregistry.info/Elements/u/P60226> ;
    reg:lexicalAlias <http://rdaregistry.info/Elements/w/verseAdaptationOfWork.en> ;
    reg:name "verseAdaptationOfWork"@en ;
    reg:status <http://metadataregistry.org/uri/RegStatus/1001> ;
    rdfs:domain <http://rdaregistry.info/Elements/c/C10001> ;
    rdfs:isDefinedBy <http://rdaregistry.info/Elements/w/> ;
    rdfs:subPropertyOf <http://rdaregistry.info/Elements/w/P10142> ;
    skos:definition "Relates a work to a work that has been adapted as a literary composition in verse form."@en .

<http://rdaregistry.info/Elements/w/P10129> a rdf:Property ;
    rdfs:label "is motion picture adaptation of (work)"@en ;
    rdakit:instructionNumber "24.5" ;
    rdakit:toolkitDefinition "A work that has been adapted as a motion picture."@en,
        "Una obra que ha sido adaptada como película cinematográfica."@es,
        "Œuvre qui a été adaptée en film."@fr ;
    rdakit:toolkitLabel "motion picture adaptation of (work)"@en,
        "adaptación cinematográfica de (obra)"@es,
        "adaptation au cinéma de (œuvre)"@fr ;
    reg:hasSubproperty <http://rdaregistry.info/Elements/w/object/P10129> ;
    reg:hasUnconstrained <http://rdaregistry.info/Elements/u/P60227> ;
    reg:lexicalAlias <http://rdaregistry.info/Elements/w/motionPictureAdaptationOfWork.en> ;
    reg:name "motionPictureAdaptationOfWork"@en ;
    reg:status <http://metadataregistry.org/uri/RegStatus/1001> ;
    rdfs:domain <http://rdaregistry.info/Elements/c/C10001> ;
    rdfs:isDefinedBy <http://rdaregistry.info/Elements/w/> ;
    rdfs:subPropertyOf <http://rdaregistry.info/Elements/w/P10142> ;
    skos:definition "Relates a work to a work that has been adapted as a motion picture."@en .

<http://rdaregistry.info/Elements/w/P10130> a rdf:Property ;
    rdfs:label "is novelization of (work)"@en ;
    rdakit:instructionNumber "24.5" ;
    rdakit:toolkitDefinition "A work that has been adapted as a novel."@en,
        "Una obra que ha sido adaptada como novela."@es,
        "Œuvre qui a été adaptée en roman."@fr ;
    rdakit:toolkitLabel "novelization of (work)"@en,
        "novelización de (obra)"@es,
        "novélisation de (œuvre)"@fr ;
    reg:hasSubproperty <http://rdaregistry.info/Elements/w/object/P10130> ;
    reg:hasUnconstrained <http://rdaregistry.info/Elements/u/P60228> ;
    reg:lexicalAlias <http://rdaregistry.info/Elements/w/novelizationOfWork.en> ;
    reg:name "novelizationOfWork"@en ;
    reg:status <http://metadataregistry.org/uri/RegStatus/1001> ;
    rdfs:domain <http://rdaregistry.info/Elements/c/C10001> ;
    rdfs:isDefinedBy <http://rdaregistry.info/Elements/w/> ;
    rdfs:subPropertyOf <http://rdaregistry.info/Elements/w/P10142> ;
    skos:definition "Relates a work to a work that has been adapted as a novel."@en .

<http://rdaregistry.info/Elements/w/P10131> a rdf:Property ;
    rdfs:label "is radio adaptation of (work)"@en ;
    rdakit:instructionNumber "24.5" ;
    rdakit:toolkitDefinition "A work that has been adapted as a radio program."@en,
        "Una obra que ha sido adaptada como programa de radio."@es,
        "Œuvre qui a été adaptée en émission de radio."@fr ;
    rdakit:toolkitLabel "radio adaptation of (work)"@en,
        "adaptación para radio de (obra)"@es,
        "adaptation pour la radio de (œuvre)"@fr ;
    reg:hasSubproperty <http://rdaregistry.info/Elements/w/object/P10131> ;
    reg:hasUnconstrained <http://rdaregistry.info/Elements/u/P60229> ;
    reg:lexicalAlias <http://rdaregistry.info/Elements/w/radioAdaptationOfWork.en> ;
    reg:name "radioAdaptationOfWork"@en ;
    reg:status <http://metadataregistry.org/uri/RegStatus/1001> ;
    rdfs:domain <http://rdaregistry.info/Elements/c/C10001> ;
    rdfs:isDefinedBy <http://rdaregistry.info/Elements/w/> ;
    rdfs:subPropertyOf <http://rdaregistry.info/Elements/w/P10142> ;
    skos:definition "Relates a work to a work that has been adapted as a radio program."@en .

<http://rdaregistry.info/Elements/w/P10132> a rdf:Property ;
    rdfs:label "is television adaptation of (work)"@en ;
    rdakit:instructionNumber "24.5" ;
    rdakit:toolkitDefinition "A work that has been adapted as a television program."@en,
        "Una obra que ha sido adaptada como programa de televisión."@es,
        "Œuvre qui a été adaptée en émission de télévision."@fr ;
    rdakit:toolkitLabel "television adaptation of (work)"@en,
        "adaptación para televisión (obra)"@es,
        "adaptation pour la télévision de (œuvre)"@fr ;
    reg:hasSubproperty <http://rdaregistry.info/Elements/w/object/P10132> ;
    reg:hasUnconstrained <http://rdaregistry.info/Elements/u/P60230> ;
    reg:lexicalAlias <http://rdaregistry.info/Elements/w/televisionAdaptationOfWork.en> ;
    reg:name "televisionAdaptationOfWork"@en ;
    reg:status <http://metadataregistry.org/uri/RegStatus/1001> ;
    rdfs:domain <http://rdaregistry.info/Elements/c/C10001> ;
    rdfs:isDefinedBy <http://rdaregistry.info/Elements/w/> ;
    rdfs:subPropertyOf <http://rdaregistry.info/Elements/w/P10142> ;
    skos:definition "Relates a work to a work that has been adapted as a television program."@en .

<http://rdaregistry.info/Elements/w/P10134> a rdf:Property ;
    rdfs:label "is motion picture screenplay based on (work)"@en ;
    rdakit:instructionNumber "24.5" ;
    rdakit:toolkitDefinition "A work that has been adapted as a screenplay for a motion picture."@en,
        "Una obra que ha sido adaptada como guión para una película cinematográfica."@es,
        "Œuvre qui a été adaptée en scénario pour un film."@fr ;
    rdakit:toolkitLabel "motion picture screenplay based on (work)"@en,
        "guión cinematográfico basado en (obra)"@es,
        "scénario de film basé sur (œuvre)"@fr ;
    reg:hasSubproperty <http://rdaregistry.info/Elements/w/object/P10134> ;
    reg:hasUnconstrained <http://rdaregistry.info/Elements/u/P60232> ;
    reg:lexicalAlias <http://rdaregistry.info/Elements/w/motionPictureScreenplayBasedOnWork.en> ;
    reg:name "motionPictureScreenplayBasedOnWork"@en ;
    reg:status <http://metadataregistry.org/uri/RegStatus/1001> ;
    rdfs:domain <http://rdaregistry.info/Elements/c/C10001> ;
    rdfs:isDefinedBy <http://rdaregistry.info/Elements/w/> ;
    rdfs:subPropertyOf <http://rdaregistry.info/Elements/w/P10133> ;
    skos:definition "Relates a work to a work that has been adapted as a screenplay for a motion picture."@en .

<http://rdaregistry.info/Elements/w/P10135> a rdf:Property ;
    rdfs:label "is television screenplay based on (work)"@en ;
    rdakit:instructionNumber "24.5" ;
    rdakit:toolkitDefinition "A work that has been adapted as a screenplay for a television program."@en,
        "Una obra que ha sido adaptada como guión para un programa de televisión."@es,
        "Œuvre qui a été adaptée en scénario pour une émission de télévision."@fr ;
    rdakit:toolkitLabel "television screenplay based on (work)"@en,
        "guión para televisión basado en (obra)"@es,
        "scénario de télévision basé sur (œuvre)"@fr ;
    reg:hasSubproperty <http://rdaregistry.info/Elements/w/object/P10135> ;
    reg:hasUnconstrained <http://rdaregistry.info/Elements/u/P60233> ;
    reg:lexicalAlias <http://rdaregistry.info/Elements/w/televisionScreenplayBasedOnWork.en> ;
    reg:name "televisionScreenplayBasedOnWork"@en ;
    reg:status <http://metadataregistry.org/uri/RegStatus/1001> ;
    rdfs:domain <http://rdaregistry.info/Elements/c/C10001> ;
    rdfs:isDefinedBy <http://rdaregistry.info/Elements/w/> ;
    rdfs:subPropertyOf <http://rdaregistry.info/Elements/w/P10133> ;
    skos:definition "Relates a work to a work that has been adapted as a screenplay for a television program."@en .

<http://rdaregistry.info/Elements/w/P10136> a rdf:Property ;
    rdfs:label "is video screenplay based on (work)"@en ;
    rdakit:instructionNumber "24.5" ;
    rdakit:toolkitDefinition "A work that has been adapted as a screenplay for a video."@en,
        "Una obra ha que ha sido adaptada como guión para un video."@es,
        "Œuvre qui a été adaptée en scénario pour une vidéo."@fr ;
    rdakit:toolkitLabel "video screenplay based on (work)"@en,
        "guión para video basado en (obra)"@es,
        "scénario de vidéo basé sur (œuvre)"@fr ;
    reg:hasSubproperty <http://rdaregistry.info/Elements/w/object/P10136> ;
    reg:hasUnconstrained <http://rdaregistry.info/Elements/u/P60234> ;
    reg:lexicalAlias <http://rdaregistry.info/Elements/w/videoScreenplayBasedOnWork.en> ;
    reg:name "videoScreenplayBasedOnWork"@en ;
    reg:status <http://metadataregistry.org/uri/RegStatus/1001> ;
    rdfs:domain <http://rdaregistry.info/Elements/c/C10001> ;
    rdfs:isDefinedBy <http://rdaregistry.info/Elements/w/> ;
    rdfs:subPropertyOf <http://rdaregistry.info/Elements/w/P10133> ;
    skos:definition "Relates a work to a work that has been adapted as a screenplay for a video."@en .

<http://rdaregistry.info/Elements/w/P10137> a rdf:Property ;
    rdfs:label "is radio script based on (work)"@en ;
    rdakit:instructionNumber "24.5" ;
    rdakit:toolkitDefinition "A work that has been adapted as a script for a radio program."@en,
        "Una obra que ha sido adaptada como guión para un programa de radio."@es,
        "Œuvre qui a été adaptée en script d’émission de radio."@fr ;
    rdakit:toolkitLabel "radio script based on (work)"@en,
        "guión radiofónico basado en (obra)"@es,
        "script radiophonique basé sur (œuvre)"@fr ;
    reg:hasSubproperty <http://rdaregistry.info/Elements/w/object/P10137> ;
    reg:hasUnconstrained <http://rdaregistry.info/Elements/u/P60235> ;
    reg:lexicalAlias <http://rdaregistry.info/Elements/w/radioScriptBasedOnWork.en> ;
    reg:name "radioScriptBasedOnWork"@en ;
    reg:status <http://metadataregistry.org/uri/RegStatus/1001> ;
    rdfs:domain <http://rdaregistry.info/Elements/c/C10001> ;
    rdfs:isDefinedBy <http://rdaregistry.info/Elements/w/> ;
    rdfs:subPropertyOf <http://rdaregistry.info/Elements/w/P10142> ;
    skos:definition "Relates a work to a work that has been adapted as a script for a radio program."@en .

<http://rdaregistry.info/Elements/w/P10138> a rdf:Property ;
    rdfs:label "is video adaptation of (work)"@en ;
    rdakit:instructionNumber "24.5" ;
    rdakit:toolkitDefinition "A work that has been adapted for video."@en,
        "Una obra que ha sido adaptada para video."@es,
        "Œuvre qui a été adaptée en vidéo."@fr ;
    rdakit:toolkitLabel "video adaptation of (work)"@en,
        "adaptación para video de (obra)"@es,
        "adaptation en vidéo de (œuvre)"@fr ;
    reg:hasSubproperty <http://rdaregistry.info/Elements/w/object/P10138> ;
    reg:hasUnconstrained <http://rdaregistry.info/Elements/u/P60236> ;
    reg:lexicalAlias <http://rdaregistry.info/Elements/w/videoAdaptationOfWork.en> ;
    reg:name "videoAdaptationOfWork"@en ;
    reg:status <http://metadataregistry.org/uri/RegStatus/1001> ;
    rdfs:domain <http://rdaregistry.info/Elements/c/C10001> ;
    rdfs:isDefinedBy <http://rdaregistry.info/Elements/w/> ;
    rdfs:subPropertyOf <http://rdaregistry.info/Elements/w/P10142> ;
    skos:definition "Relates a work to a work that has been adapted for video."@en .

<http://rdaregistry.info/Elements/w/P10139> a rdf:Property ;
    rdfs:label "is digest of (work)"@en ;
    rdakit:instructionNumber "24.5" ;
    rdakit:toolkitDefinition "A work that has been digested, i.e., systematically and comprehensively condensed."@en,
        "Una obra que ha sido resumida, i.e., condensada sistemática e integralmente."@es,
        "Œuvre qui a été condensée, c’est-à-dire abrégée de manière systématique et complète."@fr ;
    rdakit:toolkitLabel "digest of (work)"@en,
        "compendio de (obra)"@es,
        "condensé de (œuvre)"@fr ;
    reg:hasSubproperty <http://rdaregistry.info/Elements/w/object/P10139> ;
    reg:hasUnconstrained <http://rdaregistry.info/Elements/u/P60238> ;
    reg:lexicalAlias <http://rdaregistry.info/Elements/w/digestOfWork.en> ;
    reg:name "digestOfWork"@en ;
    reg:status <http://metadataregistry.org/uri/RegStatus/1001> ;
    rdfs:domain <http://rdaregistry.info/Elements/c/C10001> ;
    rdfs:isDefinedBy <http://rdaregistry.info/Elements/w/> ;
    rdfs:subPropertyOf <http://rdaregistry.info/Elements/w/P10190> ;
    skos:definition "Relates a work to a work that has been digested, i.e., systematically and comprehensively condensed."@en .

<http://rdaregistry.info/Elements/w/P10140> a rdf:Property ;
    rdfs:label "is analysis of (work)"@en ;
    rdakit:instructionNumber "23.5" ;
    rdakit:toolkitDefinition "A work that has been examined to identify its components and their relations."@en,
        "Una obra que ha sido examinada para identificar sus componentes y sus relaciones."@es,
        "Œuvre qui a été examinée pour identifier ses composantes et leurs relations."@fr ;
    rdakit:toolkitLabel "analysis of (work)"@en,
        "análisis de (obra)"@es,
        "analyse de (œuvre)"@fr ;
    reg:hasSubproperty <http://rdaregistry.info/Elements/w/object/P10140> ;
    reg:hasUnconstrained <http://rdaregistry.info/Elements/u/P60239> ;
    reg:lexicalAlias <http://rdaregistry.info/Elements/w/analysisOfWork.en> ;
    reg:name "analysisOfWork"@en ;
    reg:status <http://metadataregistry.org/uri/RegStatus/1001> ;
    rdfs:domain <http://rdaregistry.info/Elements/c/C10001> ;
    rdfs:isDefinedBy <http://rdaregistry.info/Elements/w/> ;
    rdfs:subPropertyOf <http://rdaregistry.info/Elements/w/P10100> ;
    skos:definition "Relates a work to a work that has been examined to identify its components and their relations."@en .

<http://rdaregistry.info/Elements/w/P10141> a rdf:Property ;
    rdfs:label "is series container of"@en ;
    rdakit:instructionNumber "24.5" ;
    rdakit:toolkitDefinition "A work that has been issued as part of a series."@en,
        "Una obra que se publicó como parte de una serie."@es,
        "Œuvre qui a été publiée comme partie d’une collection."@fr ;
    rdakit:toolkitLabel "series container of"@en,
        "la serie incluye (obra)"@es,
        "conteneur collection de"@fr ;
    reg:hasSubproperty <http://rdaregistry.info/Elements/w/object/P10141> ;
    reg:hasUnconstrained <http://rdaregistry.info/Elements/u/P60240> ;
    reg:lexicalAlias <http://rdaregistry.info/Elements/w/seriesContainerOf.en> ;
    reg:name "seriesContainerOf"@en ;
    reg:status <http://metadataregistry.org/uri/RegStatus/1001> ;
    rdfs:domain <http://rdaregistry.info/Elements/c/C10001> ;
    rdfs:isDefinedBy <http://rdaregistry.info/Elements/w/> ;
    rdfs:subPropertyOf <http://rdaregistry.info/Elements/w/P10147> ;
    skos:definition "Relates a work to a work that has been issued as part of a series."@en .

<http://rdaregistry.info/Elements/w/P10143> a rdf:Property ;
    rdfs:label "is free translation of (work)"@en ;
    rdakit:instructionNumber "24.5" ;
    rdakit:toolkitDefinition "A work that has been adapted and translated into another language."@en,
        "Una obra que ha sido traducida libremente, preservando el espíritu original, pero no sus detalles linguísticos."@es,
        "Œuvre qui a été librement traduite en préservant l’esprit de l’original, mais non ses particularités linguistiques."@fr ;
    rdakit:toolkitLabel "free translation of (work)"@en,
        "traducción libre de (obra)"@es,
        "traduction libre de (œuvre)"@fr ;
    reg:hasSubproperty <http://rdaregistry.info/Elements/w/object/P10143> ;
    reg:hasUnconstrained <http://rdaregistry.info/Elements/u/P60243> ;
    reg:lexicalAlias <http://rdaregistry.info/Elements/w/freeTranslationOfWork.en> ;
    reg:name "freeTranslationOfWork"@en ;
    reg:status <http://metadataregistry.org/uri/RegStatus/1001> ;
    rdfs:domain <http://rdaregistry.info/Elements/c/C10001> ;
    rdfs:isDefinedBy <http://rdaregistry.info/Elements/w/> ;
    rdfs:subPropertyOf <http://rdaregistry.info/Elements/w/P10190> ;
    skos:definition "Relates a work to a work that has been adapted and translated into another language."@en .

<http://rdaregistry.info/Elements/w/P10144> a rdf:Property ;
    rdfs:label "is parodied as (work)"@en ;
    rdakit:instructionNumber "24.5" ;
    rdakit:toolkitDefinition "A work that imitates the style or content of a source work for comic effect."@en,
        "Una obra que imita el estilo o el contenido de la obra fuente para crear un efecto cómico."@es,
        "Œuvre qui imite le style ou le contenu de l’œuvre source dans le but de produire un effet comique."@fr ;
    rdakit:toolkitLabel "parodied as (work)"@en,
        "parodiada como (obra)"@es,
        "parodié comme (œuvre)"@fr ;
    reg:hasSubproperty <http://rdaregistry.info/Elements/w/object/P10144> ;
    reg:hasUnconstrained <http://rdaregistry.info/Elements/u/P60246> ;
    reg:lexicalAlias <http://rdaregistry.info/Elements/w/parodiedAsWork.en> ;
    reg:name "parodiedAsWork"@en ;
    reg:status <http://metadataregistry.org/uri/RegStatus/1001> ;
    rdfs:domain <http://rdaregistry.info/Elements/c/C10001> ;
    rdfs:isDefinedBy <http://rdaregistry.info/Elements/w/> ;
    rdfs:subPropertyOf <http://rdaregistry.info/Elements/w/P10117> ;
    skos:definition "Relates a work to a work that imitates the style or content of a source work for comic effect."@en .

<http://rdaregistry.info/Elements/w/P10145> a rdf:Property ;
    rdfs:label "is absorbed by (work)"@en ;
    rdakit:instructionNumber "24.5" ;
    rdakit:toolkitDefinition "A work that incorporates another work."@en,
        "Una obra que incorpora otra obra."@es,
        "Œuvre qui intègre une autre œuvre."@fr ;
    rdakit:toolkitLabel "absorbed by (work)"@en,
        "absorbida por (obra)"@es,
        "absorbé par (œuvre)"@fr ;
    reg:hasSubproperty <http://rdaregistry.info/Elements/w/object/P10145> ;
    reg:hasUnconstrained <http://rdaregistry.info/Elements/u/P60247> ;
    reg:lexicalAlias <http://rdaregistry.info/Elements/w/absorbedByWork.en> ;
    reg:name "absorbedByWork"@en ;
    reg:status <http://metadataregistry.org/uri/RegStatus/1001> ;
    rdfs:domain <http://rdaregistry.info/Elements/c/C10001> ;
    rdfs:isDefinedBy <http://rdaregistry.info/Elements/w/> ;
    rdfs:subPropertyOf <http://rdaregistry.info/Elements/w/P10170> ;
    skos:definition "Relates a work to a work that incorporates another work."@en .

<http://rdaregistry.info/Elements/w/P10146> a rdf:Property ;
    rdfs:label "is absorbed in part by (work)"@en ;
    rdakit:instructionNumber "24.5" ;
    rdakit:toolkitDefinition "A work that incorporates part of the content of another work."@en,
        "Una obra que incorpora parte del contenido de otra obra."@es,
        "Œuvre qui intègre une partie du contenu d’une autre œuvre."@fr ;
    rdakit:toolkitLabel "absorbed in part by (work)"@en,
        "absorbida en parte por (obra)"@es,
        "absorbé en partie par (œuvre)"@fr ;
    reg:hasSubproperty <http://rdaregistry.info/Elements/w/object/P10146> ;
    reg:hasUnconstrained <http://rdaregistry.info/Elements/u/P60248> ;
    reg:lexicalAlias <http://rdaregistry.info/Elements/w/absorbedInPartByWork.en> ;
    reg:name "absorbedInPartByWork"@en ;
    reg:status <http://metadataregistry.org/uri/RegStatus/1001> ;
    rdfs:domain <http://rdaregistry.info/Elements/c/C10001> ;
    rdfs:isDefinedBy <http://rdaregistry.info/Elements/w/> ;
    rdfs:subPropertyOf <http://rdaregistry.info/Elements/w/P10170> ;
    skos:definition "Relates a work to a work that incorporates part of the content of another work."@en .

<http://rdaregistry.info/Elements/w/P10149> a rdf:Property ;
    rdfs:label "is errata to (work)"@en ;
    rdakit:instructionNumber "24.5" ;
    rdakit:toolkitDefinition "A work that is augmented by a list of errors in a predominant work, discovered after publication, with their corrections."@en,
        "Una obra aumentada por una lista de errores en la obra predominante, descubiertos después de la publicación, con sus correcciones."@es,
        "Œuvre qui est augmentée d’une liste d’erreurs dans l’œuvre prédominante, découvertes après publication, avec leurs corrections."@fr ;
    rdakit:toolkitLabel "errata to (work)"@en,
        "errata de (obra)"@es,
        "errata de (œuvre)"@fr ;
    reg:hasSubproperty <http://rdaregistry.info/Elements/w/object/P10149> ;
    reg:hasUnconstrained <http://rdaregistry.info/Elements/u/P60251> ;
    reg:lexicalAlias <http://rdaregistry.info/Elements/w/errataToWork.en> ;
    reg:name "errataToWork"@en ;
    reg:status <http://metadataregistry.org/uri/RegStatus/1001> ;
    rdfs:domain <http://rdaregistry.info/Elements/c/C10001> ;
    rdfs:isDefinedBy <http://rdaregistry.info/Elements/w/> ;
    rdfs:subPropertyOf <http://rdaregistry.info/Elements/w/P10192> ;
    skos:definition "Relates a work to a work that is augmented by a list of errors in a predominant work, discovered after publication, with their corrections."@en .

<http://rdaregistry.info/Elements/w/P10150> a rdf:Property ;
    rdfs:label "is guide to (work)"@en ;
    rdakit:instructionNumber "24.5" ;
    rdakit:toolkitDefinition "A work that is augmented by another work consisting of material to help the user of a predominant work, such as notes, learning and study aids, exercises, problems, questions and answers, instructor or student materials, etc."@en,
        "Una obra aumentada por otra obra que consiste en material de ayuda al usuario de la obra principal, tal como notas, ayudas para estudio y aprendizaje, ejercicios, problemas, preguntas y respuestas, materiales para el instructor o el estudiante, etc."@es,
        "Œuvre qui est augmentée par une autre œuvre consistant en documentation destinée à aider l’utilisateur de l’œuvre prédominante, telle que des notes, des outils pédagogiques, des exercices, des problèmes, des questions et réponses, du matériel didactique, etc."@fr ;
    rdakit:toolkitLabel "guide to (work)"@en,
        "guía de (obra)"@es,
        "guide de (œuvre)"@fr ;
    reg:hasSubproperty <http://rdaregistry.info/Elements/w/object/P10150> ;
    reg:hasUnconstrained <http://rdaregistry.info/Elements/u/P60252> ;
    reg:lexicalAlias <http://rdaregistry.info/Elements/w/guideToWork.en> ;
    reg:name "guideToWork"@en ;
    reg:status <http://metadataregistry.org/uri/RegStatus/1001> ;
    rdfs:domain <http://rdaregistry.info/Elements/c/C10001> ;
    rdfs:isDefinedBy <http://rdaregistry.info/Elements/w/> ;
    rdfs:subPropertyOf <http://rdaregistry.info/Elements/w/P10192> ;
    skos:definition "Relates a work to a work that is augmented by another work consisting of material, such as notes, learning and study aids, exercises, problems, questions and answers, instructor or student materials, etc., to help the user of a predominant work"@en .

<http://rdaregistry.info/Elements/w/P10151> a rdf:Property ;
    rdfs:label "is appendix to (work)"@en ;
    rdakit:instructionNumber "24.5" ;
    rdakit:toolkitDefinition "A work whose content is augmented with content from another work."@en,
        "Una obra aumentada por otra obra que consiste en material que no es esencial para la integridad del contenido, tal como una lista de referencias, tablas estadísticas y material explicativo; el material añadido puede venir al final del contenido o ser publicado separadamente."@es,
        "Œuvre qui est augmentée par une autre œuvre qui consiste en informations qui ne sont pas essentielles à la complétude du contenu, telles qu’une liste de références, des tableaux statistiques et des indications explicatives ; l’œuvre augmentante peut soit figurer à la fin du contenu, soit être publiée séparément."@fr ;
    rdakit:toolkitLabel "appendix to (work)"@en,
        "apéndice de (obra)"@es,
        "annexe de (œuvre)"@fr ;
    reg:hasSubproperty <http://rdaregistry.info/Elements/w/object/P10151> ;
    reg:hasUnconstrained <http://rdaregistry.info/Elements/u/P60253> ;
    reg:lexicalAlias <http://rdaregistry.info/Elements/w/appendixToWork.en> ;
    reg:name "appendixToWork"@en ;
    reg:status <http://metadataregistry.org/uri/RegStatus/1001> ;
    rdfs:domain <http://rdaregistry.info/Elements/c/C10001> ;
    rdfs:isDefinedBy <http://rdaregistry.info/Elements/w/> ;
    rdfs:subPropertyOf <http://rdaregistry.info/Elements/w/P10192> ;
    skos:definition "Relates a work to a work whose content is augmented with content from another work."@en ;
    skos:scopeNote "Includes lists of references, statistical tables, and explanatory matter that are not essential to the completeness of the content."@en .

<http://rdaregistry.info/Elements/w/P10152> a rdf:Property ;
    rdfs:label "is illustrations for (work)"@en ;
    rdakit:instructionNumber "24.5" ;
    rdakit:toolkitDefinition "A work that is augmented by pictorial content designed to explain or decorate it."@en,
        "Una obra aumentada con contenido pictórico diseñado para explicarla o decorarla."@es,
        "Œuvre qui est augmentée par du contenu visuel destiné à l’expliquer ou à la décorer."@fr ;
    rdakit:toolkitLabel "illustrations for (work)"@en,
        "ilustraciones para (obra)"@es,
        "illustrations pour (œuvre)"@fr ;
    reg:hasSubproperty <http://rdaregistry.info/Elements/w/object/P10152> ;
    reg:hasUnconstrained <http://rdaregistry.info/Elements/u/P60254> ;
    reg:lexicalAlias <http://rdaregistry.info/Elements/w/illustrationsForWork.en> ;
    reg:name "illustrationsForWork"@en ;
    reg:status <http://metadataregistry.org/uri/RegStatus/1001> ;
    rdfs:domain <http://rdaregistry.info/Elements/c/C10001> ;
    rdfs:isDefinedBy <http://rdaregistry.info/Elements/w/> ;
    rdfs:subPropertyOf <http://rdaregistry.info/Elements/w/P10192> ;
    skos:definition "Relates a work to a work that is augmented by pictorial content designed to explain or decorate it."@en .

<http://rdaregistry.info/Elements/w/P10153> a rdf:Property ;
    rdfs:label "is evaluation of (work)"@en ;
    rdakit:instructionNumber "23.5" ;
    rdakit:toolkitDefinition "A work that is examined or judged."@en,
        "Una obra que es examinada o juzgada."@es,
        "Œuvre qui est examinée ou jugée."@fr ;
    rdakit:toolkitLabel "evaluation of (work)"@en,
        "evaluación de (obra)"@es,
        "évaluation de (œuvre)"@fr ;
    reg:hasSubproperty <http://rdaregistry.info/Elements/w/object/P10153> ;
    reg:hasUnconstrained <http://rdaregistry.info/Elements/u/P60255> ;
    reg:lexicalAlias <http://rdaregistry.info/Elements/w/evaluationOfWork.en> ;
    reg:name "evaluationOfWork"@en ;
    reg:status <http://metadataregistry.org/uri/RegStatus/1001> ;
    rdfs:domain <http://rdaregistry.info/Elements/c/C10001> ;
    rdfs:isDefinedBy <http://rdaregistry.info/Elements/w/> ;
    rdfs:subPropertyOf <http://rdaregistry.info/Elements/w/P10100> ;
    skos:definition "Relates a work to a work that is examined or judged."@en .

<http://rdaregistry.info/Elements/w/P10154> a rdf:Property ;
    rdfs:label "is supplement to (work)"@en ;
    rdakit:instructionNumber "24.5" ;
    rdakit:toolkitDefinition "A work that is updated or otherwise complemented by an augmenting work."@en,
        "Una obra que se actualiza o complementa aumentando la obra principal."@es,
        "Œuvre qui est mise à jour ou complétée d’une autre façon par l’œuvre augmentante."@fr ;
    rdakit:toolkitLabel "supplement to (work)"@en,
        "suplemento de (obra)"@es,
        "supplément de (œuvre)"@fr ;
    reg:hasSubproperty <http://rdaregistry.info/Elements/w/object/P10154> ;
    reg:hasUnconstrained <http://rdaregistry.info/Elements/u/P60259> ;
    reg:lexicalAlias <http://rdaregistry.info/Elements/w/supplementToWork.en> ;
    reg:name "supplementToWork"@en ;
    reg:status <http://metadataregistry.org/uri/RegStatus/1001> ;
    rdfs:domain <http://rdaregistry.info/Elements/c/C10001> ;
    rdfs:isDefinedBy <http://rdaregistry.info/Elements/w/> ;
    rdfs:subPropertyOf <http://rdaregistry.info/Elements/w/P10192> ;
    skos:definition "Relates a work to a work that is updated or otherwise complemented by an augmenting work."@en .

<http://rdaregistry.info/Elements/w/P10157> a rdf:Property ;
    rdfs:label "is finding aid (work)"@en ;
    rdakit:instructionNumber "24.5" ;
    rdakit:toolkitDefinition "A work that provides a guide to the organization, arrangement, and contents of an archival collection."@en,
        "Una obra que proporciona una guía para la organización, ordenación y contenido de una colección archivística"@es,
        "Œuvre qui fournit un guide de l’organisation, du classement et du contenu d’une collection ou d’un fonds d’archives."@fr ;
    rdakit:toolkitLabel "finding aid (work)"@en,
        "guía de búsqueda de (obra)"@es,
        "instrument de recherche (œuvre)"@fr ;
    reg:hasSubproperty <http://rdaregistry.info/Elements/w/object/P10157> ;
    reg:hasUnconstrained <http://rdaregistry.info/Elements/u/P60262> ;
    reg:lexicalAlias <http://rdaregistry.info/Elements/w/findingAidWork.en> ;
    reg:name "findingAidWork"@en ;
    reg:status <http://metadataregistry.org/uri/RegStatus/1001> ;
    rdfs:domain <http://rdaregistry.info/Elements/c/C10001> ;
    rdfs:isDefinedBy <http://rdaregistry.info/Elements/w/> ;
    rdfs:subPropertyOf <http://rdaregistry.info/Elements/w/P10108> ;
    skos:definition "Relates a work to a work that provides a guide to the organization, arrangement, and contents of an archival collection."@en .

<http://rdaregistry.info/Elements/w/P10158> a rdf:Property ;
    rdfs:label "is index (work)"@en ;
    rdakit:instructionNumber "24.5" ;
    rdakit:toolkitDefinition "A work that provides a systematic, alphabetical guide to the contents of a predominant work, usually keyed to page numbers or other reference codes."@en,
        "Una obra que proporciona una guía alfabética, sistemática, al contenido de la obra principal, generalmente indicando los números de página u otros códigos de referencia"@es,
        "Œuvre qui fournit un guide méthodique et alphabétique du contenu de l’œuvre prédominante, renvoyant généralement à des numéros de page ou à d’autres codes de référence."@fr ;
    rdakit:toolkitLabel "index (work)"@en,
        "índice (obra)"@es,
        "index (œuvre)"@fr ;
    reg:hasSubproperty <http://rdaregistry.info/Elements/w/object/P10158> ;
    reg:hasUnconstrained <http://rdaregistry.info/Elements/u/P60263> ;
    reg:lexicalAlias <http://rdaregistry.info/Elements/w/indexWork.en> ;
    reg:name "indexWork"@en ;
    reg:status <http://metadataregistry.org/uri/RegStatus/1001> ;
    rdfs:domain <http://rdaregistry.info/Elements/c/C10001> ;
    rdfs:isDefinedBy <http://rdaregistry.info/Elements/w/> ;
    rdfs:subPropertyOf <http://rdaregistry.info/Elements/w/P10108> ;
    skos:definition "Relates a work to a work that provides a systematic, alphabetical guide to the contents of a predominant work, usually keyed to page numbers or other reference codes."@en .

<http://rdaregistry.info/Elements/w/P10160> a rdf:Property ;
    rdfs:label "is motion picture screenplay (work)"@en ;
    rdakit:instructionNumber "24.5" ;
    rdakit:toolkitDefinition "A work that provides text for a motion picture."@en,
        "Una obra que proporciona el texto para una película cinematográfica."@es,
        "Œuvre qui fournit le texte d’un film."@fr ;
    rdakit:toolkitLabel "motion picture screenplay (work)"@en,
        "guión cinematográfico (obra)"@es,
        "scénario de film (œuvre)"@fr ;
    reg:hasSubproperty <http://rdaregistry.info/Elements/w/object/P10160> ;
    reg:hasUnconstrained <http://rdaregistry.info/Elements/u/P60265> ;
    reg:lexicalAlias <http://rdaregistry.info/Elements/w/motionPictureScreenplayWork.en> ;
    reg:name "motionPictureScreenplayWork"@en ;
    reg:status <http://metadataregistry.org/uri/RegStatus/1001> ;
    rdfs:domain <http://rdaregistry.info/Elements/c/C10001> ;
    rdfs:isDefinedBy <http://rdaregistry.info/Elements/w/> ;
    rdfs:subPropertyOf <http://rdaregistry.info/Elements/w/P10159> ;
    skos:definition "Relates a work to a work that provides text for a motion picture."@en .

<http://rdaregistry.info/Elements/w/P10161> a rdf:Property ;
    rdfs:label "is musical setting of (work)"@en ;
    rdakit:instructionNumber "24.5" ;
    rdakit:toolkitDefinition "A work that provides text for a non-dramatic musical work, other than an oratorio."@en,
        "Una obra que proporciona el texto de una obra musical no dramática, diferente del oratorio."@es,
        "Œuvre qui fournit le texte d’une œuvre musicale non théâtrale, autre qu’un oratorio."@fr ;
    rdakit:toolkitLabel "musical setting of (work)"@en,
        "composición musical de (obra)"@es,
        "mise en musique de (œuvre)"@fr ;
    reg:hasSubproperty <http://rdaregistry.info/Elements/w/object/P10161> ;
    reg:hasUnconstrained <http://rdaregistry.info/Elements/u/P60266> ;
    reg:lexicalAlias <http://rdaregistry.info/Elements/w/musicalSettingOfWork.en> ;
    reg:name "musicalSettingOfWork"@en ;
    reg:status <http://metadataregistry.org/uri/RegStatus/1001> ;
    rdfs:domain <http://rdaregistry.info/Elements/c/C10001> ;
    rdfs:isDefinedBy <http://rdaregistry.info/Elements/w/> ;
    rdfs:subPropertyOf <http://rdaregistry.info/Elements/w/P10190> ;
    skos:definition "Relates a work to a work that provides text for a non-dramatic musical work, other than an oratorio."@en .

<http://rdaregistry.info/Elements/w/P10162> a rdf:Property ;
    rdfs:label "is radio script (work)"@en ;
    rdakit:instructionNumber "24.5" ;
    rdakit:toolkitDefinition "A work that provides text for a radio program."@en,
        "Una obra que proporciona el texto para un programa de radio."@es,
        "Œuvre qui fournit le texte d’une émission de radio."@fr ;
    rdakit:toolkitLabel "radio script (work)"@en,
        "guión radiofónico (obra)"@es,
        "script radiophonique (œuvre)"@fr ;
    reg:hasSubproperty <http://rdaregistry.info/Elements/w/object/P10162> ;
    reg:hasUnconstrained <http://rdaregistry.info/Elements/u/P60267> ;
    reg:lexicalAlias <http://rdaregistry.info/Elements/w/radioScriptWork.en> ;
    reg:name "radioScriptWork"@en ;
    reg:status <http://metadataregistry.org/uri/RegStatus/1001> ;
    rdfs:domain <http://rdaregistry.info/Elements/c/C10001> ;
    rdfs:isDefinedBy <http://rdaregistry.info/Elements/w/> ;
    rdfs:subPropertyOf <http://rdaregistry.info/Elements/w/P10103> ;
    skos:definition "Relates a work to a work that provides text for a radio program."@en .

<http://rdaregistry.info/Elements/w/P10163> a rdf:Property ;
    rdfs:label "is television screenplay (work)"@en ;
    rdakit:instructionNumber "24.5" ;
    rdakit:toolkitDefinition "A work that provides text for a television program."@en,
        "Una obra que proporciona el texto para un programa de televisión."@es,
        "Œuvre qui fournit le texte d’une émission de télévision."@fr ;
    rdakit:toolkitLabel "television screenplay (work)"@en,
        "guión de televisión (obra)"@es,
        "scénario de télévision (œuvre)"@fr ;
    reg:hasSubproperty <http://rdaregistry.info/Elements/w/object/P10163> ;
    reg:hasUnconstrained <http://rdaregistry.info/Elements/u/P60268> ;
    reg:lexicalAlias <http://rdaregistry.info/Elements/w/televisionScreenplayWork.en> ;
    reg:name "televisionScreenplayWork"@en ;
    reg:status <http://metadataregistry.org/uri/RegStatus/1001> ;
    rdfs:domain <http://rdaregistry.info/Elements/c/C10001> ;
    rdfs:isDefinedBy <http://rdaregistry.info/Elements/w/> ;
    rdfs:subPropertyOf <http://rdaregistry.info/Elements/w/P10159> ;
    skos:definition "Relates a work to a work that provides text for a television program."@en .

<http://rdaregistry.info/Elements/w/P10164> a rdf:Property ;
    rdfs:label "is video screenplay (work)"@en ;
    rdakit:instructionNumber "24.5" ;
    rdakit:toolkitDefinition "A work that provides text for a video."@en,
        "Una obra que proporciona el texto para un video."@es,
        "Œuvre qui fournit le texte d’une vidéo."@fr ;
    rdakit:toolkitLabel "video screenplay (work)"@en,
        "guión de video (obra)"@es,
        "scénario de vidéo (œuvre)"@fr ;
    reg:hasSubproperty <http://rdaregistry.info/Elements/w/object/P10164> ;
    reg:hasUnconstrained <http://rdaregistry.info/Elements/u/P60269> ;
    reg:lexicalAlias <http://rdaregistry.info/Elements/w/videoScreenplayWork.en> ;
    reg:name "videoScreenplayWork"@en ;
    reg:status <http://metadataregistry.org/uri/RegStatus/1001> ;
    rdfs:domain <http://rdaregistry.info/Elements/c/C10001> ;
    rdfs:isDefinedBy <http://rdaregistry.info/Elements/w/> ;
    rdfs:subPropertyOf <http://rdaregistry.info/Elements/w/P10159> ;
    skos:definition "Relates a work to a work that provides text for a video."@en .

<http://rdaregistry.info/Elements/w/P10165> a rdf:Property ;
    rdfs:label "is libretto (work)"@en ;
    rdakit:instructionNumber "24.5" ;
    rdakit:toolkitDefinition "A work that provides the text of an opera or other work for the musical stage, or an oratorio."@en,
        "Una obra que proporciona el texto de una ópera u otra obra para representación musical, o un oratorio."@es,
        "Œuvre qui fournit le texte d’un opéra ou d’une autre œuvre pour la scène musicale, ou bien d’un oratorio."@fr ;
    rdakit:toolkitLabel "libretto (work)"@en,
        "libreto (obra)"@es,
        "livret (œuvre)"@fr ;
    reg:hasSubproperty <http://rdaregistry.info/Elements/w/object/P10165> ;
    reg:hasUnconstrained <http://rdaregistry.info/Elements/u/P60270> ;
    reg:lexicalAlias <http://rdaregistry.info/Elements/w/librettoWork.en> ;
    reg:name "librettoWork"@en ;
    reg:status <http://metadataregistry.org/uri/RegStatus/1001> ;
    rdfs:domain <http://rdaregistry.info/Elements/c/C10001> ;
    rdfs:isDefinedBy <http://rdaregistry.info/Elements/w/> ;
    rdfs:subPropertyOf <http://rdaregistry.info/Elements/w/P10103> ;
    skos:definition "Relates a work to a work that provides the text of an opera or other work for the musical stage, or an oratorio."@en .

<http://rdaregistry.info/Elements/w/P10166> a rdf:Property ;
    rdfs:label "is paraphrased as (work)"@en ;
    rdakit:instructionNumber "24.5" ;
    rdakit:toolkitDefinition "A work that restates the content of a source work in a different form."@en,
        "Una obra que replantea el contenido de la obra fuente en una forma diferente."@es,
        "Œuvre qui reprend le contenu de l’œuvre source sous une formulation différente."@fr ;
    rdakit:toolkitLabel "paraphrased as (work)"@en,
        "parafraseada como (obra)"@es,
        "paraphrasé comme (œuvre)"@fr ;
    reg:hasSubproperty <http://rdaregistry.info/Elements/w/object/P10166> ;
    reg:hasUnconstrained <http://rdaregistry.info/Elements/u/P60273> ;
    reg:lexicalAlias <http://rdaregistry.info/Elements/w/paraphrasedAsWork.en> ;
    reg:name "paraphrasedAsWork"@en ;
    reg:status <http://metadataregistry.org/uri/RegStatus/1001> ;
    rdfs:domain <http://rdaregistry.info/Elements/c/C10001> ;
    rdfs:isDefinedBy <http://rdaregistry.info/Elements/w/> ;
    rdfs:subPropertyOf <http://rdaregistry.info/Elements/w/P10148> ;
    skos:definition "Relates a work to a work that restates the content of a source work in a different form."@en .

<http://rdaregistry.info/Elements/w/P10167> a rdf:Property ;
    rdfs:label "is abridged as (work)"@en ;
    rdakit:instructionNumber "24.5" ;
    rdakit:toolkitDefinition "A work that shortens a source work without changing the general meaning or manner of presentation."@en,
        "Una obra que acorta el contenido de la obra fuente sin cambiar el significado general o la manera de presentación."@es,
        "Œuvre qui raccourcit l’œuvre source sans en changer le sens général ou le mode de présentation."@fr ;
    rdakit:toolkitLabel "abridged as (work)"@en,
        "abreviada como (obra)"@es,
        "abrégé comme (œuvre)"@fr ;
    reg:hasSubproperty <http://rdaregistry.info/Elements/w/object/P10167> ;
    reg:hasUnconstrained <http://rdaregistry.info/Elements/u/P60275> ;
    reg:lexicalAlias <http://rdaregistry.info/Elements/w/abridgedAsWork.en> ;
    reg:name "abridgedAsWork"@en ;
    reg:status <http://metadataregistry.org/uri/RegStatus/1001> ;
    rdfs:domain <http://rdaregistry.info/Elements/c/C10001> ;
    rdfs:isDefinedBy <http://rdaregistry.info/Elements/w/> ;
    rdfs:subPropertyOf <http://rdaregistry.info/Elements/w/P10148> ;
    skos:definition "Relates a work to a work that shortens a source work without changing the general meaning or manner of presentation."@en .

<http://rdaregistry.info/Elements/w/P10168> a rdf:Property ;
    rdfs:label "is continuation in part of (work)"@en ;
    rdakit:instructionNumber "24.5" ;
    rdakit:toolkitDefinition "A work that split into two or more separate works with new titles."@en,
        "Una obra que se divide en dos o más obras separadas con títulos nuevos."@es,
        "Œuvre qui s’est scindée en deux ou plusieurs œuvres distinctes avec de nouveaux titres."@fr ;
    rdakit:toolkitLabel "continuation in part of (work)"@en,
        "continúa en parte (obra)"@es,
        "continuation partielle de (œuvre)"@fr ;
    reg:hasSubproperty <http://rdaregistry.info/Elements/w/object/P10168> ;
    reg:hasUnconstrained <http://rdaregistry.info/Elements/u/P60276> ;
    reg:lexicalAlias <http://rdaregistry.info/Elements/w/continuationInPartOfWork.en> ;
    reg:name "continuationInPartOfWork"@en ;
    reg:status <http://metadataregistry.org/uri/RegStatus/1001> ;
    rdfs:domain <http://rdaregistry.info/Elements/c/C10001> ;
    rdfs:isDefinedBy <http://rdaregistry.info/Elements/w/> ;
    rdfs:subPropertyOf <http://rdaregistry.info/Elements/w/P10156> ;
    skos:definition "Relates a work to a work that split into two or more separate works with new titles."@en ;
    skos:scopeNote "This relationship applies generally to serials."@en .

<http://rdaregistry.info/Elements/w/P10169> a rdf:Property ;
    rdfs:label "is separated from (work)"@en ;
    rdakit:instructionNumber "24.5" ;
    rdakit:toolkitDefinition "A work that spun off a part of its content to form a new work."@en,
        "Una obra que se desprende de una parte de su contenido para formar una obra nueva."@es,
        "Œuvre dont une partie du contenu a été détachée pour former une nouvelle œuvre."@fr ;
    rdakit:toolkitLabel "separated from (work)"@en,
        "separada de (obra)"@es,
        "scission de (œuvre)"@fr ;
    reg:hasSubproperty <http://rdaregistry.info/Elements/w/object/P10169> ;
    reg:hasUnconstrained <http://rdaregistry.info/Elements/u/P60277> ;
    reg:lexicalAlias <http://rdaregistry.info/Elements/w/separatedFromWork.en> ;
    reg:name "separatedFromWork"@en ;
    reg:status <http://metadataregistry.org/uri/RegStatus/1001> ;
    rdfs:domain <http://rdaregistry.info/Elements/c/C10001> ;
    rdfs:isDefinedBy <http://rdaregistry.info/Elements/w/> ;
    rdfs:subPropertyOf <http://rdaregistry.info/Elements/w/P10156> ;
    skos:definition "Relates a work to a work that spun off a part of its content to form a new work."@en .

<http://rdaregistry.info/Elements/w/P10171> a rdf:Property ;
    rdfs:label "is digested as (work)"@en ;
    rdakit:instructionNumber "24.5" ;
    rdakit:toolkitDefinition "A work that systematically and comprehensively condenses a source work."@en,
        "Una obra que condensa sistemática e integralmente la obra fuente."@es,
        "Œuvre qui abrège de manière systématique et complète l’œuvre source."@fr ;
    rdakit:toolkitLabel "digested as (work)"@en,
        "compendiada como (obra)"@es,
        "condensé comme (œuvre)"@fr ;
    reg:hasSubproperty <http://rdaregistry.info/Elements/w/object/P10171> ;
    reg:hasUnconstrained <http://rdaregistry.info/Elements/u/P60279> ;
    reg:lexicalAlias <http://rdaregistry.info/Elements/w/digestedAsWork.en> ;
    reg:name "digestedAsWork"@en ;
    reg:status <http://metadataregistry.org/uri/RegStatus/1001> ;
    rdfs:domain <http://rdaregistry.info/Elements/c/C10001> ;
    rdfs:isDefinedBy <http://rdaregistry.info/Elements/w/> ;
    rdfs:subPropertyOf <http://rdaregistry.info/Elements/w/P10148> ;
    skos:definition "Relates a work to a work that systematically and comprehensively condenses a source work."@en .

<http://rdaregistry.info/Elements/w/P10172> a rdf:Property ;
    rdfs:label "is supplement (work)"@en ;
    rdakit:instructionNumber "24.5" ;
    rdakit:toolkitDefinition "A work that updates or otherwise complements a predominant work."@en,
        "Una obra que actualiza o complementa la obra predominante."@es,
        "Œuvre qui met à jour ou complète d’une autre façon l’œuvre prédominante."@fr ;
    rdakit:toolkitLabel "supplement (work)"@en,
        "suplemento (obra)"@es,
        "supplément (œuvre)"@fr ;
    reg:hasSubproperty <http://rdaregistry.info/Elements/w/object/P10172> ;
    reg:hasUnconstrained <http://rdaregistry.info/Elements/u/P60281> ;
    reg:lexicalAlias <http://rdaregistry.info/Elements/w/supplementWork.en> ;
    reg:name "supplementWork"@en ;
    reg:status <http://metadataregistry.org/uri/RegStatus/1001> ;
    rdfs:domain <http://rdaregistry.info/Elements/c/C10001> ;
    rdfs:isDefinedBy <http://rdaregistry.info/Elements/w/> ;
    rdfs:subPropertyOf <http://rdaregistry.info/Elements/w/P10108> ;
    skos:definition "Relates a work to a work that updates or otherwise complements a predominant work."@en .

<http://rdaregistry.info/Elements/w/P10173> a rdf:Property ;
    rdfs:label "is screenplay for motion picture (work)"@en ;
    rdakit:instructionNumber "24.5" ;
    rdakit:toolkitDefinition "A work that uses the text as a screenplay for a motion picture."@en,
        "Una obra que utiliza el texto como guión para una película cinematográfica."@es,
        "Œuvre qui utilise le texte comme scénario d’un film."@fr ;
    rdakit:toolkitLabel "screenplay for motion picture (work)"@en,
        "guión para película cinematográfica (obra)"@es,
        "scénario pour le film (œuvre)"@fr ;
    reg:hasSubproperty <http://rdaregistry.info/Elements/w/object/P10173> ;
    reg:hasUnconstrained <http://rdaregistry.info/Elements/u/P60282> ;
    reg:lexicalAlias <http://rdaregistry.info/Elements/w/screenplayForTheMotionPictureWork.en> ;
    reg:name "screenplayForTheMotionPictureWork"@en ;
    reg:status <http://metadataregistry.org/uri/RegStatus/1001> ;
    rdfs:domain <http://rdaregistry.info/Elements/c/C10001> ;
    rdfs:isDefinedBy <http://rdaregistry.info/Elements/w/> ;
    rdfs:subPropertyOf <http://rdaregistry.info/Elements/w/P10105> ;
    skos:definition "Relates a work to a work that uses the text as a screenplay for a motion picture."@en .

<http://rdaregistry.info/Elements/w/P10174> a rdf:Property ;
    rdfs:label "is screenplay for television program (work)"@en ;
    rdakit:instructionNumber "24.5" ;
    rdakit:toolkitDefinition "A work that uses the text as a screenplay for a television program."@en,
        "Una obra que utiliza el texto como guión para un programa de televisión."@es,
        "Œuvre qui utilise le texte comme scénario d’une émission de télévision."@fr ;
    rdakit:toolkitLabel "screenplay for television program (work)"@en,
        "guión para programa de televisión (obra)"@es,
        "scénario pour l’émission de télévision (œuvre)"@fr ;
    reg:hasSubproperty <http://rdaregistry.info/Elements/w/object/P10174> ;
    reg:hasUnconstrained <http://rdaregistry.info/Elements/u/P60283> ;
    reg:lexicalAlias <http://rdaregistry.info/Elements/w/screenplayForTheTelevisionProgramWork.en> ;
    reg:name "screenplayForTheTelevisionProgramWork"@en ;
    reg:status <http://metadataregistry.org/uri/RegStatus/1001> ;
    rdfs:domain <http://rdaregistry.info/Elements/c/C10001> ;
    rdfs:isDefinedBy <http://rdaregistry.info/Elements/w/> ;
    rdfs:subPropertyOf <http://rdaregistry.info/Elements/w/P10105> ;
    skos:definition "Relates a work to a work that uses the text as a screenplay for a television program."@en .

<http://rdaregistry.info/Elements/w/P10175> a rdf:Property ;
    rdfs:label "is screenplay for video (work)"@en ;
    rdakit:instructionNumber "24.5" ;
    rdakit:toolkitDefinition "A work that uses the text as a screenplay for a video."@en,
        "Una obra que utiliza el texto como guión para un vídeo."@es,
        "Œuvre qui utilise le texte comme scénario d’une vidéo."@fr ;
    rdakit:toolkitLabel "screenplay for video (work)"@en,
        "guión para programa de vídeo (obra)"@es,
        "scénario pour la vidéo (œuvre)"@fr ;
    reg:hasSubproperty <http://rdaregistry.info/Elements/w/object/P10175> ;
    reg:hasUnconstrained <http://rdaregistry.info/Elements/u/P60284> ;
    reg:lexicalAlias <http://rdaregistry.info/Elements/w/screenplayForTheVideoWork.en> ;
    reg:name "screenplayForTheVideoWork"@en ;
    reg:status <http://metadataregistry.org/uri/RegStatus/1001> ;
    rdfs:domain <http://rdaregistry.info/Elements/c/C10001> ;
    rdfs:isDefinedBy <http://rdaregistry.info/Elements/w/> ;
    rdfs:subPropertyOf <http://rdaregistry.info/Elements/w/P10105> ;
    skos:definition "Relates a work to a work that uses the text as a screenplay for a video."@en .

<http://rdaregistry.info/Elements/w/P10176> a rdf:Property ;
    rdfs:label "is script for radio program (work)"@en ;
    rdakit:instructionNumber "24.5" ;
    rdakit:toolkitDefinition "A work that uses the text as a script for a radio program."@en,
        "Una obra que utiliza el texto como guión para un programa de radio."@es,
        "Œuvre qui utilise le texte comme script d’une émission de radio."@fr ;
    rdakit:toolkitLabel "script for radio program (work)"@en,
        "guión para programa de radio (obra)"@es,
        "script pour l’émission de radio (œuvre)"@fr ;
    reg:hasSubproperty <http://rdaregistry.info/Elements/w/object/P10176> ;
    reg:hasUnconstrained <http://rdaregistry.info/Elements/u/P60285> ;
    reg:lexicalAlias <http://rdaregistry.info/Elements/w/scriptForTheRadioProgramWork.en> ;
    reg:name "scriptForTheRadioProgramWork"@en ;
    reg:status <http://metadataregistry.org/uri/RegStatus/1001> ;
    rdfs:domain <http://rdaregistry.info/Elements/c/C10001> ;
    rdfs:isDefinedBy <http://rdaregistry.info/Elements/w/> ;
    rdfs:subPropertyOf <http://rdaregistry.info/Elements/w/P10103> ;
    skos:definition "Relates a work to a work that uses the text as a script for a radio program."@en .

<http://rdaregistry.info/Elements/w/P10177> a rdf:Property ;
    rdfs:label "is addenda to (work)"@en ;
    rdakit:instructionNumber "24.5" ;
    rdakit:toolkitDefinition "A work whose content is completed with brief content from another work."@en,
        "Una obra a la cual se añade material adicional breve, menos extenso que un suplemento, pero esencial para la integridad del contenido de la obra; generalmente se agrega al final de la obra, pero en algunos casos se publica separadamente."@es,
        "Œuvre à laquelle sont ajoutées de brèves informations additionnelles, moins étendues qu’un supplément, mais essentielles à la complétude du contenu de l’œuvre ; ces informations sont généralement ajoutées à la fin de l’œuvre, mais peuvent aussi parfois être publiées séparément."@fr ;
    rdakit:toolkitLabel "addenda to (work)"@en,
        "adenda de (obra)"@es,
        "addenda de (œuvre)"@fr ;
    reg:hasSubproperty <http://rdaregistry.info/Elements/w/object/P10177> ;
    reg:hasUnconstrained <http://rdaregistry.info/Elements/u/P60286> ;
    reg:lexicalAlias <http://rdaregistry.info/Elements/w/addendaToWork.en> ;
    reg:name "addendaToWork"@en ;
    reg:status <http://metadataregistry.org/uri/RegStatus/1001> ;
    rdfs:domain <http://rdaregistry.info/Elements/c/C10001> ;
    rdfs:isDefinedBy <http://rdaregistry.info/Elements/w/> ;
    rdfs:subPropertyOf <http://rdaregistry.info/Elements/w/P10192> ;
    skos:definition "Relates a work to a work whose content is completed with brief content from another work."@en .

<http://rdaregistry.info/Elements/w/P10178> a rdf:Property ;
    rdfs:label "is review of (work)"@en ;
    rdakit:instructionNumber "23.5" ;
    rdakit:toolkitDefinition "A work used as a basis for a brief evaluation."@en,
        "Una obra que es usada como base para una evaluación breve."@es,
        "Œuvre servant de base à une brève évaluation."@fr ;
    rdakit:toolkitLabel "review of (work)"@en,
        "reseña de (obra)"@es,
        "recension de (œuvre)"@fr ;
    reg:hasSubproperty <http://rdaregistry.info/Elements/w/object/P10178> ;
    reg:hasUnconstrained <http://rdaregistry.info/Elements/u/P60288> ;
    reg:lexicalAlias <http://rdaregistry.info/Elements/w/reviewOfWork.en> ;
    reg:name "reviewOfWork"@en ;
    reg:status <http://metadataregistry.org/uri/RegStatus/1001> ;
    rdfs:domain <http://rdaregistry.info/Elements/c/C10001> ;
    rdfs:isDefinedBy <http://rdaregistry.info/Elements/w/> ;
    rdfs:subPropertyOf <http://rdaregistry.info/Elements/w/P10100> ;
    skos:definition "Relates a work to a work used as a basis for a brief evaluation."@en .

<http://rdaregistry.info/Elements/w/P10179> a rdf:Property ;
    rdfs:label "is summary of (work)"@en ;
    rdakit:instructionNumber "24.5" ;
    rdakit:toolkitDefinition "A work used as a basis for a brief recapitulation of its content."@en,
        "Una obra utilizada como base para una recapitulación breve de su contenido."@es,
        "Œuvre servant de base à une brève récapitulation de son contenu."@fr ;
    rdakit:toolkitLabel "summary of (work)"@en,
        "sumario de (obra)"@es,
        "résumé de (œuvre)"@fr ;
    reg:hasSubproperty <http://rdaregistry.info/Elements/w/object/P10179> ;
    reg:hasUnconstrained <http://rdaregistry.info/Elements/u/P60289> ;
    reg:lexicalAlias <http://rdaregistry.info/Elements/w/summaryOfWork.en> ;
    reg:name "summaryOfWork"@en ;
    reg:status <http://metadataregistry.org/uri/RegStatus/1001> ;
    rdfs:domain <http://rdaregistry.info/Elements/c/C10001> ;
    rdfs:isDefinedBy <http://rdaregistry.info/Elements/w/> ;
    rdfs:subPropertyOf <http://rdaregistry.info/Elements/w/P10190> ;
    skos:definition "Relates a work to a work used as a basis for a brief recapitulation of its content."@en .

<http://rdaregistry.info/Elements/w/P10180> a rdf:Property ;
    rdfs:label "is catalogue of (work)"@en ;
    rdakit:instructionNumber "24.5" ;
    rdakit:toolkitDefinition "A work used as a basis for a catalogue, i.e., a complete enumeration of items arranged systematically."@en,
        "Una obra utilizada como base de un catálogo, i.e., una enumeración total de ítems ordenados sistemáticamente."@es,
        "Œuvre servant de base à un catalogue, c’est-à-dire une énumération complète des items classés systématiquement."@fr ;
    rdakit:toolkitLabel "catalogue of (work)"@en,
        "catálogo de (obra)"@es,
        "catalogue de (œuvre)"@fr ;
    reg:hasSubproperty <http://rdaregistry.info/Elements/w/object/P10180> ;
    reg:hasUnconstrained <http://rdaregistry.info/Elements/u/P60290> ;
    reg:lexicalAlias <http://rdaregistry.info/Elements/w/catalogueOfWork.en> ;
    reg:name "catalogueOfWork"@en ;
    reg:status <http://metadataregistry.org/uri/RegStatus/1001> ;
    rdfs:domain <http://rdaregistry.info/Elements/c/C10001> ;
    rdfs:isDefinedBy <http://rdaregistry.info/Elements/w/> ;
    rdfs:subPropertyOf <http://rdaregistry.info/Elements/w/P10192> ;
    skos:definition "Relates a work to a work used as a basis for a catalogue, i.e., a complete enumeration of items arranged systematically."@en .

<http://rdaregistry.info/Elements/w/P10181> a rdf:Property ;
    rdfs:label "is concordance to (work)"@en ;
    rdakit:instructionNumber "24.5" ;
    rdakit:toolkitDefinition "A work used as a basis for a concordance, i.e., an index of all the words in a predominant work."@en,
        "Una obra utilizada como base de una concordancia, i.e., un índice de todas las palabras en la obra principal."@es,
        "Œuvre servant de base à une concordance, c’est-à-dire un index de tous les mots de l’œuvre prédominante."@fr ;
    rdakit:toolkitLabel "concordance to (work)"@en,
        "concordancia de (obra)"@es,
        "concordance de (œuvre)"@fr ;
    reg:hasSubproperty <http://rdaregistry.info/Elements/w/object/P10181> ;
    reg:hasUnconstrained <http://rdaregistry.info/Elements/u/P60291> ;
    reg:lexicalAlias <http://rdaregistry.info/Elements/w/concordanceToWork.en> ;
    reg:name "concordanceToWork"@en ;
    reg:status <http://metadataregistry.org/uri/RegStatus/1001> ;
    rdfs:domain <http://rdaregistry.info/Elements/c/C10001> ;
    rdfs:isDefinedBy <http://rdaregistry.info/Elements/w/> ;
    rdfs:subPropertyOf <http://rdaregistry.info/Elements/w/P10192> ;
    skos:definition "Relates a work to a work used as a basis for a concordance, i.e., an index of all the words in the predominant work."@en .

<http://rdaregistry.info/Elements/w/P10182> a rdf:Property ;
    rdfs:label "is critique of (work)"@en ;
    rdakit:instructionNumber "23.5" ;
    rdakit:toolkitDefinition "A work used as a basis for a critical evaluation."@en,
        "Una obra usada como base de una evaluación crítica."@es,
        "Œuvre servant de base à une évaluation critique."@fr ;
    rdakit:toolkitLabel "critique of (work)"@en,
        "crítica de (obra)"@es,
        "critique de (œuvre)"@fr ;
    reg:hasSubproperty <http://rdaregistry.info/Elements/w/object/P10182> ;
    reg:hasUnconstrained <http://rdaregistry.info/Elements/u/P60292> ;
    reg:lexicalAlias <http://rdaregistry.info/Elements/w/critiqueOfWork.en> ;
    reg:name "critiqueOfWork"@en ;
    reg:status <http://metadataregistry.org/uri/RegStatus/1001> ;
    rdfs:domain <http://rdaregistry.info/Elements/c/C10001> ;
    rdfs:isDefinedBy <http://rdaregistry.info/Elements/w/> ;
    rdfs:subPropertyOf <http://rdaregistry.info/Elements/w/P10100> ;
    skos:definition "Relates a work to a work used as a basis for a critical evaluation."@en .

<http://rdaregistry.info/Elements/w/P10183> a rdf:Property ;
    rdfs:label "is choreographic adaptation of (work)"@en ;
    rdakit:instructionNumber "24.5" ;
    rdakit:toolkitDefinition "A work used that has been adapted as a work consisting of movement."@en,
        "Una obra que ha sido adaptada como una obra que consiste en movimiento (p. ej., danza)."@es,
        "Œuvre qui a été adaptée en œuvre consistant en mouvement (par exemple, de la danse)."@fr ;
    rdakit:toolkitLabel "choreographic adaptation of (work)"@en,
        "adaptación coreográfica de (obra)"@es,
        "adaptation chorégraphique de (œuvre)"@fr ;
    reg:hasSubproperty <http://rdaregistry.info/Elements/w/object/P10183> ;
    reg:hasUnconstrained <http://rdaregistry.info/Elements/u/P60293> ;
    reg:lexicalAlias <http://rdaregistry.info/Elements/w/choreographicAdaptationOfWork.en> ;
    reg:name "choreographicAdaptationOfWork"@en ;
    reg:status <http://metadataregistry.org/uri/RegStatus/1001> ;
    rdfs:domain <http://rdaregistry.info/Elements/c/C10001> ;
    rdfs:isDefinedBy <http://rdaregistry.info/Elements/w/> ;
    rdfs:subPropertyOf <http://rdaregistry.info/Elements/w/P10142> ;
    skos:definition "Relates a work to a work that has been adapted as a work consisting of movement."@en .

<http://rdaregistry.info/Elements/w/P10184> a rdf:Property ;
    rdfs:label "is expanded version of (work)"@en ;
    rdakit:instructionNumber "24.5" ;
    rdakit:toolkitDefinition "A work used as a basis for a derivative work that enlarges upon the content of a source work."@en,
        "Una obra utilizada como base para una obra derivada que aumenta el contenido de la obra fuente."@es,
        "Œuvre servant de base à une œuvre dérivée qui accroît le contenu de l’œuvre source."@fr ;
    rdakit:toolkitLabel "expanded version of (work)"@en,
        "versión ampliada de (obra)"@es,
        "version augmentée de (œuvre)"@fr ;
    reg:hasSubproperty <http://rdaregistry.info/Elements/w/object/P10184> ;
    reg:hasUnconstrained <http://rdaregistry.info/Elements/u/P60294> ;
    reg:lexicalAlias <http://rdaregistry.info/Elements/w/expandedVersionOfWork.en> ;
    reg:name "expandedVersionOfWork"@en ;
    reg:status <http://metadataregistry.org/uri/RegStatus/1001> ;
    rdfs:domain <http://rdaregistry.info/Elements/c/C10001> ;
    rdfs:isDefinedBy <http://rdaregistry.info/Elements/w/> ;
    rdfs:subPropertyOf <http://rdaregistry.info/Elements/w/P10190> ;
    skos:definition "Relates a work to a work used as a basis for a derivative work that enlarges upon the content of a source work."@en .

<http://rdaregistry.info/Elements/w/P10185> a rdf:Property ;
    rdfs:label "is remake of (work)"@en ;
    rdakit:instructionNumber "24.5" ;
    rdakit:toolkitDefinition "A work used as a basis for a new motion picture, radio program, television program, or video."@en,
        "Una obra utilizada como base para nueva película cinematográfica, programa de radio, programa de televisión o video."@es,
        "Œuvre servant de base à un nouveau film, une nouvelle émission de radio, une nouvelle émission de télévision ou une nouvelle vidéo."@fr ;
    rdakit:toolkitLabel "remake of (work)"@en,
        "remake de (obra)"@es,
        "nouvelle version de (œuvre)"@fr ;
    reg:hasSubproperty <http://rdaregistry.info/Elements/w/object/P10185> ;
    reg:hasUnconstrained <http://rdaregistry.info/Elements/u/P60295> ;
    reg:lexicalAlias <http://rdaregistry.info/Elements/w/remakeOfWork.en> ;
    reg:name "remakeOfWork"@en ;
    reg:status <http://metadataregistry.org/uri/RegStatus/1001> ;
    rdfs:domain <http://rdaregistry.info/Elements/c/C10001> ;
    rdfs:isDefinedBy <http://rdaregistry.info/Elements/w/> ;
    rdfs:subPropertyOf <http://rdaregistry.info/Elements/w/P10190> ;
    skos:definition "Relates a work to a work used as a basis for a new motion picture, radio program, television program, or video."@en .

<http://rdaregistry.info/Elements/w/P10186> a rdf:Property ;
    rdfs:label "is paraphrase of (work)"@en ;
    rdakit:instructionNumber "24.5" ;
    rdakit:toolkitDefinition "A work used as a basis for a paraphrase, i.e., a restating of the content of a source work in a different form."@en,
        "Una obra utilizada como base para una paráfrasis, i.e., un replanteamiento del contenido de la obra fuente en una forma diferente."@es,
        "Œuvre servant de base à une paraphrase, c’est-à-dire une reprise du contenu de l’œuvre source sous une formulation différente."@fr ;
    rdakit:toolkitLabel "paraphrase of (work)"@en,
        "paráfrasis de (obra)"@es,
        "paraphrase de (œuvre)"@fr ;
    reg:hasSubproperty <http://rdaregistry.info/Elements/w/object/P10186> ;
    reg:hasUnconstrained <http://rdaregistry.info/Elements/u/P60296> ;
    reg:lexicalAlias <http://rdaregistry.info/Elements/w/paraphraseOfWork.en> ;
    reg:name "paraphraseOfWork"@en ;
    reg:status <http://metadataregistry.org/uri/RegStatus/1001> ;
    rdfs:domain <http://rdaregistry.info/Elements/c/C10001> ;
    rdfs:isDefinedBy <http://rdaregistry.info/Elements/w/> ;
    rdfs:subPropertyOf <http://rdaregistry.info/Elements/w/P10190> ;
    skos:definition "Relates a work to a work used as a basis for a paraphrase, i.e., a restating of the content of a source work in a different form."@en .

<http://rdaregistry.info/Elements/w/P10187> a rdf:Property ;
    rdfs:label "is commentary on (work)"@en ;
    rdakit:instructionNumber "23.5" ;
    rdakit:toolkitDefinition "A work used as a basis for a set of explanatory or critical notes."@en,
        "Una obra usada como base para un conjunto de notas explicativas o críticas."@es,
        "Œuvre servant de base à un ensemble de notes explicatives ou critiques."@fr ;
    rdakit:toolkitLabel "commentary on (work)"@en,
        "comentario sobre (obra)"@es,
        "commentaire sur (œuvre)"@fr ;
    reg:hasSubproperty <http://rdaregistry.info/Elements/w/object/P10187> ;
    reg:hasUnconstrained <http://rdaregistry.info/Elements/u/P60298> ;
    reg:lexicalAlias <http://rdaregistry.info/Elements/w/commentaryOnWork.en> ;
    reg:name "commentaryOnWork"@en ;
    reg:status <http://metadataregistry.org/uri/RegStatus/1001> ;
    rdfs:domain <http://rdaregistry.info/Elements/c/C10001> ;
    rdfs:isDefinedBy <http://rdaregistry.info/Elements/w/> ;
    rdfs:subPropertyOf <http://rdaregistry.info/Elements/w/P10100> ;
    skos:definition "Relates a work to a work used as a basis for a set of explanatory or critical notes."@en .

<http://rdaregistry.info/Elements/w/P10188> a rdf:Property ;
    rdfs:label "is index to (work)"@en ;
    rdakit:instructionNumber "24.5" ;
    rdakit:toolkitDefinition "A work used as a basis for an index, i.e., a systematic, alphabetical guide to the contents of a predominant work, usually keyed to page numbers or other reference codes."@en,
        "Una obra utilizada como base para un índice, i.e., una guía sistemática, alfabética al contenido de la obra principal, generalmente indicando los números de página u otros códigos de referencia."@es,
        "Œuvre servant de base à un index, c’est-à-dire un guide méthodique et alphabétique du contenu de l’œuvre prédominante, renvoyant généralement à des numéros de page ou à d’autres codes de référence."@fr ;
    rdakit:toolkitLabel "index to (work)"@en,
        "índice de (obra)"@es,
        "index de (œuvre)"@fr ;
    reg:hasSubproperty <http://rdaregistry.info/Elements/w/object/P10188> ;
    reg:hasUnconstrained <http://rdaregistry.info/Elements/u/P60302> ;
    reg:lexicalAlias <http://rdaregistry.info/Elements/w/indexToWork.en> ;
    reg:name "indexToWork"@en ;
    reg:status <http://metadataregistry.org/uri/RegStatus/1001> ;
    rdfs:domain <http://rdaregistry.info/Elements/c/C10001> ;
    rdfs:isDefinedBy <http://rdaregistry.info/Elements/w/> ;
    rdfs:subPropertyOf <http://rdaregistry.info/Elements/w/P10192> ;
    skos:definition "Relates a work to a work used as a basis for an index, i.e., a systematic, alphabetical guide to the contents of a predominant work, usually keyed to page numbers or other reference codes."@en .

<http://rdaregistry.info/Elements/w/P10189> a rdf:Property ;
    rdfs:label "is libretto based on (work)"@en ;
    rdakit:instructionNumber "24.5" ;
    rdakit:toolkitDefinition "A work used as the basis for the text of an opera or other work for the musical stage, or an oratorio."@en,
        "Una obra utilizada como base para el texto de una ópera u otra obra para escenario musical o un oratorio."@es,
        "Œuvre servant de base au texte d’un opéra ou d’une autre œuvre pour la scène musicale, ou bien d’un oratorio."@fr ;
    rdakit:toolkitLabel "libretto based on (work)"@en,
        "libreto basado en (obra)"@es,
        "livret basé sur (œuvre)"@fr ;
    reg:hasSubproperty <http://rdaregistry.info/Elements/w/object/P10189> ;
    reg:hasUnconstrained <http://rdaregistry.info/Elements/u/P60304> ;
    reg:lexicalAlias <http://rdaregistry.info/Elements/w/librettoBasedOnWork.en> ;
    reg:name "librettoBasedOnWork"@en ;
    reg:status <http://metadataregistry.org/uri/RegStatus/1001> ;
    rdfs:domain <http://rdaregistry.info/Elements/c/C10001> ;
    rdfs:isDefinedBy <http://rdaregistry.info/Elements/w/> ;
    rdfs:subPropertyOf <http://rdaregistry.info/Elements/w/P10142> ;
    skos:definition "Relates a work to a work that has been adapted as the text of an opera or other work for the musical stage, or an oratorio."@en .

<http://rdaregistry.info/Elements/w/P10191> a rdf:Property ;
    rdfs:label "is continued by (work)"@en ;
    rdakit:instructionNumber "24.5" ;
    rdakit:toolkitDefinition "A work whose content continues an earlier work."@en,
        "Una obra cuyo contenido continúa una obra anterior bajo un título nuevo."@es,
        "Œuvre dont le contenu continue une œuvre antérieure."@fr ;
    rdakit:toolkitLabel "continued by (work)"@en,
        "continuada por (obra)"@es,
        "continué par (œuvre)"@fr ;
    reg:hasSubproperty <http://rdaregistry.info/Elements/w/object/P10191> ;
    reg:hasUnconstrained <http://rdaregistry.info/Elements/u/P60306> ;
    reg:lexicalAlias <http://rdaregistry.info/Elements/w/continuedByWork.en> ;
    reg:name "continuedByWork"@en ;
    reg:status <http://metadataregistry.org/uri/RegStatus/1001> ;
    rdfs:domain <http://rdaregistry.info/Elements/c/C10001> ;
    rdfs:isDefinedBy <http://rdaregistry.info/Elements/w/> ;
    rdfs:subPropertyOf <http://rdaregistry.info/Elements/w/P10170> ;
    skos:definition "Relates a work to a work whose content continues an earlier work."@en ;
    skos:scopeNote "This relationship applies generally to serials."@en .

<http://rdaregistry.info/Elements/w/P10193> a rdf:Property ;
    rdfs:label "is abstracts for (work)"@en ;
    rdakit:instructionNumber "24.5" ;
    rdakit:toolkitDefinition "A work whose contents have been abstracted by an abstracting and indexing service."@en,
        "Una obra cuyo contenido ha sido resumido por un servicio de indización y resumenes."@es,
        "Œuvre dont le contenu a été résumé par un service d’analyse et d’indexation."@fr ;
    rdakit:toolkitLabel "abstracts for (work)"@en,
        "resúmenes de (obra)"@es,
        "résumés analytiques pour (œuvre)"@fr ;
    reg:hasSubproperty <http://rdaregistry.info/Elements/w/object/P10193> ;
    reg:hasUnconstrained <http://rdaregistry.info/Elements/u/P60308> ;
    reg:lexicalAlias <http://rdaregistry.info/Elements/w/abstractsForWork.en> ;
    reg:name "abstractsForWork"@en ;
    reg:status <http://metadataregistry.org/uri/RegStatus/1001> ;
    rdfs:domain <http://rdaregistry.info/Elements/c/C10001> ;
    rdfs:isDefinedBy <http://rdaregistry.info/Elements/w/> ;
    rdfs:subPropertyOf <http://rdaregistry.info/Elements/w/P10190> ;
    skos:definition "Relates a work to a work whose contents have been abstracted by an abstracting and indexing service."@en .

<http://rdaregistry.info/Elements/w/P10194> a rdf:Property ;
    rdfs:label "is indexing for (work)"@en ;
    rdakit:instructionNumber "24.5" ;
    rdakit:toolkitDefinition "A work whose contents have been indexed by an abstracting and indexing service."@en,
        "Una obra cuyo contenido ha sido indizado por un servicio de indización y resumenes."@es,
        "Œuvre dont le contenu a été indexé par un service d’analyse et d’indexation."@fr ;
    rdakit:toolkitLabel "indexing for (work)"@en,
        "indización de (obra)"@es,
        "indexation pour (œuvre)"@fr ;
    reg:hasSubproperty <http://rdaregistry.info/Elements/w/object/P10194> ;
    reg:hasUnconstrained <http://rdaregistry.info/Elements/u/P60309> ;
    reg:lexicalAlias <http://rdaregistry.info/Elements/w/indexingForWork.en> ;
    reg:name "indexingForWork"@en ;
    reg:status <http://metadataregistry.org/uri/RegStatus/1001> ;
    rdfs:domain <http://rdaregistry.info/Elements/c/C10001> ;
    rdfs:isDefinedBy <http://rdaregistry.info/Elements/w/> ;
    rdfs:subPropertyOf <http://rdaregistry.info/Elements/w/P10190> ;
    skos:definition "Relates a work to a work whose contents have been indexed by an abstracting and indexing service."@en .

<http://rdaregistry.info/Elements/w/P10195> a rdf:Property ;
    rdfs:label "is prequel to"@en ;
    rdakit:instructionNumber "24.5" ;
    rdakit:toolkitDefinition "A work whose narrative is extended backwards in time by a later work."@en,
        "Una obra cuya narración se extiende hacia atrás en el tiempo por una obra posterior."@es,
        "Œuvre dont le récit est étendu sur une période plus ancienne dans le temps par l’œuvre ultérieure."@fr ;
    rdakit:toolkitLabel "prequel to"@en,
        "precuela de"@es,
        "antépisode de"@fr ;
    reg:hasSubproperty <http://rdaregistry.info/Elements/w/object/P10195> ;
    reg:hasUnconstrained <http://rdaregistry.info/Elements/u/P60310> ;
    reg:lexicalAlias <http://rdaregistry.info/Elements/w/prequelTo.en> ;
    reg:name "prequelTo"@en ;
    reg:status <http://metadataregistry.org/uri/RegStatus/1001> ;
    rdfs:domain <http://rdaregistry.info/Elements/c/C10001> ;
    rdfs:isDefinedBy <http://rdaregistry.info/Elements/w/> ;
    rdfs:subPropertyOf <http://rdaregistry.info/Elements/w/P10170> ;
    skos:definition "Relates a work to a work whose narrative is extended backwards in time by a later work."@en .

<http://rdaregistry.info/Elements/w/P10197> a rdf:Property ;
    rdfs:label "is parody of (work)"@en ;
    rdakit:instructionNumber "24.5" ;
    rdakit:toolkitDefinition "A work whose style or content is imitated for comic effect."@en,
        "Una obra cuyo estilo o contenido es imitado para obtener un efecto cómico."@es,
        "Œuvre dont le style ou le contenu est imité dans le but de produire un effet comique."@fr ;
    rdakit:toolkitLabel "parody of (work)"@en,
        "parodia de (obra)"@es,
        "parodie de (œuvre)"@fr ;
    reg:hasSubproperty <http://rdaregistry.info/Elements/w/object/P10197> ;
    reg:hasUnconstrained <http://rdaregistry.info/Elements/u/P60312> ;
    reg:lexicalAlias <http://rdaregistry.info/Elements/w/parodyOfWork.en> ;
    reg:name "parodyOfWork"@en ;
    reg:status <http://metadataregistry.org/uri/RegStatus/1001> ;
    rdfs:domain <http://rdaregistry.info/Elements/c/C10001> ;
    rdfs:isDefinedBy <http://rdaregistry.info/Elements/w/> ;
    rdfs:subPropertyOf <http://rdaregistry.info/Elements/w/P10196> ;
    skos:definition "Relates a work to a work whose style or content is imitated for comic effect."@en .

<http://rdaregistry.info/Elements/w/P10200> a rdf:Property ;
    rdfs:label "has landscape architect"@en ;
    rdakit:instructionNumber "18.5" ;
    rdakit:toolkitDefinition "An architect responsible for creating landscape works."@en,
        "Un arquitecto responsable de la creación de obras paisajísticas."@es,
        "Architecte responsable de la création d’œuvres paysagères."@fr ;
    rdakit:toolkitLabel "landscape architect"@en,
        "arquitecto paisajista"@es,
        "architecte paysagiste"@fr ;
    reg:hasSubproperty <http://rdaregistry.info/Elements/w/object/P10200> ;
    reg:hasUnconstrained <http://rdaregistry.info/Elements/u/P60473> ;
    reg:lexicalAlias <http://rdaregistry.info/Elements/w/landscapeArchitect.en> ;
    reg:name "landscapeArchitect"@en ;
    reg:status <http://metadataregistry.org/uri/RegStatus/1001> ;
    rdfs:domain <http://rdaregistry.info/Elements/c/C10001> ;
    rdfs:isDefinedBy <http://rdaregistry.info/Elements/w/> ;
    rdfs:subPropertyOf <http://rdaregistry.info/Elements/w/P10062> ;
    skos:definition "Relates a work to an architect responsible for creating landscape works."@en .

<http://rdaregistry.info/Elements/w/P10201> a rdf:Property ;
    rdfs:label "is finding aid for (work)"@en ;
    rdakit:instructionNumber "24.5" ;
    rdakit:toolkitDefinition "An archival collection that is described in a finding aid, i.e., a guide to the organization, arrangement, and contents of a collection."@en,
        "Una colección de archivo que está descrita en una ayuda de búsqueda, i.e., una guía a la organización, ordenación y contenido de la colección."@es,
        "Collection ou fonds d’archives qui est décrit dans un instrument de recherche, c’est-à-dire un guide de l’organisation, du classement et du contenu de la collection ou du fonds."@fr ;
    rdakit:toolkitLabel "finding aid for (work)"@en,
        "guía de búsqueda de (obra)"@es,
        "instrument de recherche pour (œuvre)"@fr ;
    reg:hasSubproperty <http://rdaregistry.info/Elements/w/object/P10201> ;
    reg:hasUnconstrained <http://rdaregistry.info/Elements/u/P60474> ;
    reg:lexicalAlias <http://rdaregistry.info/Elements/w/findingAidForWork.en> ;
    reg:name "findingAidForWork"@en ;
    reg:status <http://metadataregistry.org/uri/RegStatus/1001> ;
    rdfs:domain <http://rdaregistry.info/Elements/c/C10001> ;
    rdfs:isDefinedBy <http://rdaregistry.info/Elements/w/> ;
    rdfs:subPropertyOf <http://rdaregistry.info/Elements/w/P10192> ;
    skos:definition "Relates a work to an archival collection that is described in a finding aid, i.e., a guide to the organization, arrangement, and contents of a collection."@en .

<http://rdaregistry.info/Elements/w/P10202> a rdf:Property ;
    rdfs:label "has sculptor"@en ;
    rdakit:instructionNumber "18.5" ;
    rdakit:toolkitDefinition "An artist responsible for creating a three-dimensional work by modeling, carving, or similar technique."@en,
        "Un artista responsable de la creación de una obra tridimensional mediante modelado, tallado o técnica similar."@es,
        "Artiste responsable de la création d’une œuvre tridimensionnelle par le modelage, la taille ou une technique similaire."@fr ;
    rdakit:toolkitLabel "sculptor"@en,
        "escultor"@es,
        "sculpteur"@fr ;
    reg:hasSubproperty <http://rdaregistry.info/Elements/w/object/P10202> ;
    reg:hasUnconstrained <http://rdaregistry.info/Elements/u/P60475> ;
    reg:lexicalAlias <http://rdaregistry.info/Elements/w/sculptor.en> ;
    reg:name "sculptor"@en ;
    reg:status <http://metadataregistry.org/uri/RegStatus/1001> ;
    rdfs:domain <http://rdaregistry.info/Elements/c/C10001> ;
    rdfs:isDefinedBy <http://rdaregistry.info/Elements/w/> ;
    rdfs:subPropertyOf <http://rdaregistry.info/Elements/w/P10058> ;
    skos:definition "Relates a work to an artist responsible for creating a three-dimensional work by modeling, carving, or similar technique."@en .

<http://rdaregistry.info/Elements/w/P10203> a rdf:Property ;
    rdfs:label "has screenwriter"@en ;
    rdakit:instructionNumber "18.5" ;
    rdakit:toolkitDefinition "An author of a screenplay, script, or scene."@en,
        "Un autor de un guión o escena."@es,
        "Auteur d’un scénario, d’un script ou d’une scène."@fr ;
    rdakit:toolkitLabel "screenwriter"@en,
        "guionista"@es,
        "scénariste"@fr ;
    reg:hasSubproperty <http://rdaregistry.info/Elements/w/object/P10203> ;
    reg:hasUnconstrained <http://rdaregistry.info/Elements/u/P60476> ;
    reg:lexicalAlias <http://rdaregistry.info/Elements/w/screenwriter.en> ;
    reg:name "screenwriter"@en ;
    reg:status <http://metadataregistry.org/uri/RegStatus/1001> ;
    rdfs:domain <http://rdaregistry.info/Elements/c/C10001> ;
    rdfs:isDefinedBy <http://rdaregistry.info/Elements/w/> ;
    rdfs:subPropertyOf <http://rdaregistry.info/Elements/w/P10061> ;
    skos:definition "Relates a work to an author of a screenplay, script, or scene."@en .

<http://rdaregistry.info/Elements/w/P10206> a rdf:Property ;
    rdfs:label "is replacement in part of (work)"@en ;
    rdakit:instructionNumber "24.5" ;
    rdakit:toolkitDefinition "An earlier work whose content has been partially replaced by a later work, usually because the later work contains updated or new information that makes the earlier work obsolete."@en,
        "Una obra anterior cuyo contenido ha sido reemplazado parcialmente por una obra posterior, generalmente porque la obra posterior contiene información actualizada o nueva que hace obsoleta la obra anterior."@es,
        "Œuvre antérieure dont le contenu a été partiellement remplacé par une œuvre ultérieure, généralement parce que l’œuvre ultérieure contient de l’information nouvelle ou mise à jour qui rend l’œuvre antérieure obsolète."@fr ;
    rdakit:toolkitLabel "replacement in part of (work)"@en,
        "reemplazo en parte de (obra)"@es,
        "remplacement partiel de (œuvre)"@fr ;
    reg:hasSubproperty <http://rdaregistry.info/Elements/w/object/P10206> ;
    reg:hasUnconstrained <http://rdaregistry.info/Elements/u/P60479> ;
    reg:lexicalAlias <http://rdaregistry.info/Elements/w/replacementInPartOfWork.en> ;
    reg:name "replacementInPartOfWork"@en ;
    reg:status <http://metadataregistry.org/uri/RegStatus/1001> ;
    rdfs:domain <http://rdaregistry.info/Elements/c/C10001> ;
    rdfs:isDefinedBy <http://rdaregistry.info/Elements/w/> ;
    rdfs:subPropertyOf <http://rdaregistry.info/Elements/w/P10156> ;
    skos:definition "Relates a work to an earlier work whose content has been partially replaced by a later work, usually because the later work contains updated or new information that makes the earlier work obsolete."@en ;
    skos:scopeNote "This relationship applies generally to single-part units, multipart monographs, and integrating resources."@en .

<http://rdaregistry.info/Elements/w/P10207> a rdf:Property ;
    rdfs:label "is replacement of (work)"@en ;
    rdakit:instructionNumber "24.5" ;
    rdakit:toolkitDefinition "An earlier work whose content has been replaced by a later work, usually because the later work contains updated or new information that makes the earlier work obsolete."@en,
        "Una obra anterior cuyo contenido ha sido reemplazado por una obra posterior, generalmente porque la obra posterior contiene información actualizada o nueva que hace obsoleta la obra anterior."@es,
        "Œuvre antérieure dont le contenu a été remplacé par une œuvre ultérieure, généralement parce que l’œuvre ultérieure contient de l’information nouvelle ou mise à jour qui rend l’œuvre antérieure obsolète."@fr ;
    rdakit:toolkitLabel "replacement of (work)"@en,
        "reemplazo de (obra)"@es,
        "remplacement de (œuvre)"@fr ;
    reg:hasSubproperty <http://rdaregistry.info/Elements/w/object/P10207> ;
    reg:hasUnconstrained <http://rdaregistry.info/Elements/u/P60480> ;
    reg:lexicalAlias <http://rdaregistry.info/Elements/w/replacementOfWork.en> ;
    reg:name "replacementOfWork"@en ;
    reg:status <http://metadataregistry.org/uri/RegStatus/1001> ;
    rdfs:domain <http://rdaregistry.info/Elements/c/C10001> ;
    rdfs:isDefinedBy <http://rdaregistry.info/Elements/w/> ;
    rdfs:subPropertyOf <http://rdaregistry.info/Elements/w/P10156> ;
    skos:definition "Relates a work to an earlier work whose content has been replaced by a later work, usually because the later work contains updated or new information that makes the earlier work obsolete."@en ;
    skos:scopeNote "This relationship applies generally to single-part units, multipart monographs, and integrating resources."@en .

<http://rdaregistry.info/Elements/w/P10211> a rdf:Property ;
    rdfs:label "is split into (work)"@en ;
    rdakit:instructionNumber "24.5" ;
    rdakit:toolkitDefinition "A work resulting from division of an earlier work into two or more separate works."@en,
        "Una de dos o más obras que resultan de la división de una obra anterior en obras separadas."@es,
        "L’une de deux ou plusieurs œuvres résultant de la division d’une œuvre antérieure en œuvres séparées."@fr ;
    rdakit:toolkitLabel "split into (work)"@en,
        "escindida en (obra)"@es,
        "scindé en (œuvre)"@fr ;
    reg:hasSubproperty <http://rdaregistry.info/Elements/w/object/P10211> ;
    reg:hasUnconstrained <http://rdaregistry.info/Elements/u/P60503> ;
    reg:lexicalAlias <http://rdaregistry.info/Elements/w/splitIntoWork.en> ;
    reg:name "splitIntoWork"@en ;
    reg:status <http://metadataregistry.org/uri/RegStatus/1001> ;
    rdfs:domain <http://rdaregistry.info/Elements/c/C10001> ;
    rdfs:isDefinedBy <http://rdaregistry.info/Elements/w/> ;
    rdfs:subPropertyOf <http://rdaregistry.info/Elements/w/P10170> ;
    skos:definition "Relates a work to a work resulting from division of an earlier work into two or more separate works."@en .

<http://rdaregistry.info/Elements/w/P10212> a rdf:Property ;
    rdfs:label "is merged to form (work)"@en ;
    rdakit:instructionNumber "24.5" ;
    rdakit:toolkitDefinition "A work formed from the coming together of two or more works."@en,
        "Una obra formada the unión de dos o más obras."@es,
        "Œuvre formée par l’assemblage de deux ou plusieurs œuvres."@fr ;
    rdakit:toolkitLabel "merged to form (work)"@en,
        "fusionada para formar (obra)"@es,
        "fusionné pour former (œuvre)"@fr ;
    reg:hasSubproperty <http://rdaregistry.info/Elements/w/object/P10212> ;
    reg:hasUnconstrained <http://rdaregistry.info/Elements/u/P60504> ;
    reg:lexicalAlias <http://rdaregistry.info/Elements/w/mergedToFormWork.en> ;
    reg:name "mergedToFormWork"@en ;
    reg:status <http://metadataregistry.org/uri/RegStatus/1001> ;
    rdfs:domain <http://rdaregistry.info/Elements/c/C10001> ;
    rdfs:isDefinedBy <http://rdaregistry.info/Elements/w/> ;
    rdfs:subPropertyOf <http://rdaregistry.info/Elements/w/P10170> ;
    skos:definition "Relates a work to a work formed from the coming together of two or more works."@en .

<http://rdaregistry.info/Elements/w/P10213> a rdf:Property ;
    rdfs:label "is merger of (work)"@en ;
    rdakit:instructionNumber "24.5" ;
    rdakit:toolkitDefinition "A work that came together with one or more other works to form a new work."@en,
        "Una obra que viene con una o más obras para formar la nueva obra."@es,
        "Œuvre qui s’est assemblée avec une ou plusieurs autres œuvres pour former la nouvelle œuvre."@fr ;
    rdakit:toolkitLabel "merger of (work)"@en,
        "fusión de (obra)"@es,
        "fusion de (œuvre)"@fr ;
    reg:hasSubproperty <http://rdaregistry.info/Elements/w/object/P10213> ;
    reg:hasUnconstrained <http://rdaregistry.info/Elements/u/P60505> ;
    reg:lexicalAlias <http://rdaregistry.info/Elements/w/mergerOfWork.en> ;
    reg:name "mergerOfWork"@en ;
    reg:status <http://metadataregistry.org/uri/RegStatus/1001> ;
    rdfs:domain <http://rdaregistry.info/Elements/c/C10001> ;
    rdfs:isDefinedBy <http://rdaregistry.info/Elements/w/> ;
    rdfs:subPropertyOf <http://rdaregistry.info/Elements/w/P10156> ;
    skos:definition "Relates a work to a work that came together with one or more other works to form a new work."@en .

<http://rdaregistry.info/Elements/w/P10223> a rdf:Property ;
    rdfs:label "has preferred title for work"@en,
        "har föredragen titel för verket"@sv ;
    rdakit:instructionNumber "6.2.2" ;
    rdakit:toolkitDefinition "A title or form of title chosen to identify a work."@en,
        "El título o forma del título elegido para identificar la obra."@es,
        "Le titre ou la forme de titre choisie pour identifier l’œuvre."@fr ;
    rdakit:toolkitLabel "preferred title for work"@en,
        "título preferido de la obra"@es,
        "titre privilégié de l’œuvre"@fr,
        "föredragen titel för verket"@sv ;
    reg:hasUnconstrained <http://rdaregistry.info/Elements/u/P60588> ;
    reg:lexicalAlias <http://rdaregistry.info/Elements/w/preferredTitleForWork.en> ;
    reg:name "preferredTitleForWork"@en ;
    reg:status <http://metadataregistry.org/uri/RegStatus/1001> ;
    rdfs:domain <http://rdaregistry.info/Elements/c/C10001> ;
    rdfs:isDefinedBy <http://rdaregistry.info/Elements/w/> ;
    rdfs:subPropertyOf <http://rdaregistry.info/Elements/w/P10088> ;
    skos:definition "Relates a work to a title or form of title chosen to identify a work."@en ;
    skos:scopeNote "The preferred title is also the basis for an authorized access point representing that work."@en,
        "Le titre privilégié constitue aussi l’élément de base du point d’accès autorisé représentant cette œuvre."@fr .

<http://rdaregistry.info/Elements/w/P10224> a rdf:Property ;
    rdfs:label "is absorption of (work)"@en ;
    rdakit:instructionNumber "24.5" ;
    rdakit:toolkitDefinition "A work that has been incorporated into another work."@en,
        "La obra que se ha incorporado en otra obra."@es,
        "L’œuvre qui a été intégrée dans une autre œuvre."@fr ;
    rdakit:toolkitLabel "absorption of (work)"@en,
        "absorbida (obra)"@es,
        "absorption de (œuvre)"@fr ;
    reg:hasSubproperty <http://rdaregistry.info/Elements/w/object/P10224> ;
    reg:hasUnconstrained <http://rdaregistry.info/Elements/u/P60574> ;
    reg:lexicalAlias <http://rdaregistry.info/Elements/w/absorptionOfWork.en> ;
    reg:name "absorptionOfWork"@en ;
    reg:status <http://metadataregistry.org/uri/RegStatus/1001> ;
    rdfs:domain <http://rdaregistry.info/Elements/c/C10001> ;
    rdfs:isDefinedBy <http://rdaregistry.info/Elements/w/> ;
    rdfs:subPropertyOf <http://rdaregistry.info/Elements/w/P10156> ;
    skos:definition "Relates a work to a work that has been incorporated into another work."@en .

<http://rdaregistry.info/Elements/w/P10225> a rdf:Property ;
    rdfs:label "is absorption in part of (work)"@en ;
    rdakit:instructionNumber "24.5" ;
    rdakit:toolkitDefinition "A work that has been partially incorporated into another work."@en,
        "Una obra que incorpora parte del contenido de otra obra."@es,
        "L’œuvre qui a été partiellement intégrée dans une autre œuvre."@fr ;
    rdakit:toolkitLabel "absorption in part of (work)"@en,
        "absorbida en parte por (obra)"@es,
        "absorption partielle de (œuvre)"@fr ;
    reg:hasSubproperty <http://rdaregistry.info/Elements/w/object/P10225> ;
    reg:hasUnconstrained <http://rdaregistry.info/Elements/u/P60575> ;
    reg:lexicalAlias <http://rdaregistry.info/Elements/w/absorptionInPartOfWork.en> ;
    reg:name "absorptionInPartOfWork"@en ;
    reg:status <http://metadataregistry.org/uri/RegStatus/1001> ;
    rdfs:domain <http://rdaregistry.info/Elements/c/C10001> ;
    rdfs:isDefinedBy <http://rdaregistry.info/Elements/w/> ;
    rdfs:subPropertyOf <http://rdaregistry.info/Elements/w/P10156> ;
    skos:definition "Relates a work to a work that has been partially incorporated into another work."@en .

<http://rdaregistry.info/Elements/w/P10226> a rdf:Property ;
    rdfs:label "is continuation of (work)"@en ;
    rdakit:instructionNumber "24.5" ;
    rdakit:toolkitDefinition "A work that is continued by the content of a later work."@en,
        "La obra que es continuada por el contenido de una obra posterior."@es,
        "Œuvre qui est continuée par le contenu d’une œuvre ultérieure."@fr ;
    rdakit:toolkitLabel "continuation of (work)"@en,
        "continuación de(obra)"@es,
        "continuation de (œuvre)"@fr ;
    reg:hasSubproperty <http://rdaregistry.info/Elements/w/object/P10226> ;
    reg:hasUnconstrained <http://rdaregistry.info/Elements/u/P60576> ;
    reg:lexicalAlias <http://rdaregistry.info/Elements/w/continuationOfWork.en> ;
    reg:name "continuationOfWork"@en ;
    reg:status <http://metadataregistry.org/uri/RegStatus/1001> ;
    rdfs:domain <http://rdaregistry.info/Elements/c/C10001> ;
    rdfs:isDefinedBy <http://rdaregistry.info/Elements/w/> ;
    rdfs:subPropertyOf <http://rdaregistry.info/Elements/w/P10156> ;
    skos:definition "Relates a work to a work that is continued by the content of a later work."@en ;
    skos:scopeNote "This relationship applies generally to serials."@en .

<http://rdaregistry.info/Elements/w/P10227> a rdf:Property ;
    rdfs:label "is sequel to"@en ;
    rdakit:instructionNumber "24.5" ;
    rdakit:toolkitDefinition "A work whose narrative is continued by a later work."@en,
        "La obra cuya narración se continúa en una obra posterior."@es,
        "L’œuvre dont le récit est continué par l’œuvre ultérieure."@fr ;
    rdakit:toolkitLabel "sequel to"@en,
        "secuela de"@es,
        "suite de"@fr ;
    reg:hasSubproperty <http://rdaregistry.info/Elements/w/object/P10227> ;
    reg:hasUnconstrained <http://rdaregistry.info/Elements/u/P60577> ;
    reg:lexicalAlias <http://rdaregistry.info/Elements/w/sequelTo.en> ;
    reg:name "sequelTo"@en ;
    reg:status <http://metadataregistry.org/uri/RegStatus/1001> ;
    rdfs:domain <http://rdaregistry.info/Elements/c/C10001> ;
    rdfs:isDefinedBy <http://rdaregistry.info/Elements/w/> ;
    rdfs:subPropertyOf <http://rdaregistry.info/Elements/w/P10156> ;
    skos:definition "Relates a work to a work whose narrative is continued by a later work."@en .

<http://rdaregistry.info/Elements/w/P10233> a rdf:Property ;
    rdfs:label "is musical theatre adaptation of (work)"@en ;
    rdakit:instructionNumber "24.5" ;
    rdakit:toolkitDefinition "A work that has been adapted as a musical theatre work."@en,
        "Una obra que ha sido adaptada como una obra de teatro musical."@es,
        "Œuvre qui a été adaptée en œuvre de théâtre musical."@fr ;
    rdakit:toolkitLabel "musical theatre adaptation of (work)"@en,
        "adaptación a teatro musical de (obra)"@es,
        "adaptation au théâtre musical de (œuvre)"@fr ;
    reg:hasSubproperty <http://rdaregistry.info/Elements/w/object/P10233> ;
    reg:hasUnconstrained <http://rdaregistry.info/Elements/u/P60719> ;
    reg:lexicalAlias <http://rdaregistry.info/Elements/w/musicalTheatreAdaptationOfWork.en> ;
    reg:name "musicalTheatreAdaptationOfWork"@en ;
    reg:status <http://metadataregistry.org/uri/RegStatus/1001> ;
    rdfs:domain <http://rdaregistry.info/Elements/c/C10001> ;
    rdfs:isDefinedBy <http://rdaregistry.info/Elements/w/> ;
    rdfs:subPropertyOf <http://rdaregistry.info/Elements/w/P10142> ;
    skos:definition "Relates a work to a work that has been adapted as a musical theatre work."@en .

<http://rdaregistry.info/Elements/w/P10234> a rdf:Property ;
    rdfs:label "is opera adaptation of (work)"@en ;
    rdakit:instructionNumber "24.5" ;
    rdakit:toolkitDefinition "A work that has been adapted as opera."@en,
        "Una obra que ha sido adaptada como ópera."@es,
        "Œuvre qui a été adaptée à l’opéra."@fr ;
    rdakit:toolkitLabel "opera adaptation of (work)"@en,
        "adaptación a la ópera (obra)"@es,
        "adaptation à l’opéra de (œuvre)"@fr ;
    reg:hasSubproperty <http://rdaregistry.info/Elements/w/object/P10234> ;
    reg:hasUnconstrained <http://rdaregistry.info/Elements/u/P60720> ;
    reg:lexicalAlias <http://rdaregistry.info/Elements/w/operaAdaptationOf.en> ;
    reg:name "operaAdaptationOf"@en ;
    reg:status <http://metadataregistry.org/uri/RegStatus/1001> ;
    rdfs:domain <http://rdaregistry.info/Elements/c/C10001> ;
    rdfs:isDefinedBy <http://rdaregistry.info/Elements/w/> ;
    rdfs:subPropertyOf <http://rdaregistry.info/Elements/w/P10142> ;
    skos:definition "Relates a work to a work that has been adapted as an opera."@en .

<http://rdaregistry.info/Elements/w/P10235> a rdf:Property ;
    rdfs:label "is adapted as musical theatre (work)"@en ;
    rdakit:instructionNumber "24.5" ;
    rdakit:toolkitDefinition "A musical theatre work based on a source work."@en,
        "Una obra de teatro musical basada en la obra fuente."@es,
        "Œuvre de théâtre musical basée sur l’œuvre source."@fr ;
    rdakit:toolkitLabel "adapted as musical theatre (work)"@en,
        "adaptada como teatro musical (obra)"@es,
        "adapté au théâtre musical (œuvre)"@fr ;
    reg:hasSubproperty <http://rdaregistry.info/Elements/w/object/P10235> ;
    reg:hasUnconstrained <http://rdaregistry.info/Elements/u/P60721> ;
    reg:lexicalAlias <http://rdaregistry.info/Elements/w/adaptedAsMusicalTheatreWork.en> ;
    reg:name "adaptedAsMusicalTheatreWork"@en ;
    reg:status <http://metadataregistry.org/uri/RegStatus/1001> ;
    rdfs:domain <http://rdaregistry.info/Elements/c/C10001> ;
    rdfs:isDefinedBy <http://rdaregistry.info/Elements/w/> ;
    rdfs:subPropertyOf <http://rdaregistry.info/Elements/w/P10155> ;
    skos:definition "Relates a work to a musical theatre work based on a source work."@en .

<http://rdaregistry.info/Elements/w/P10236> a rdf:Property ;
    rdfs:label "is adapted as opera (work)"@en ;
    rdakit:instructionNumber "24.5" ;
    rdakit:toolkitDefinition "An opera based on a source work."@en,
        "Una ópera basada en la obra fuente."@es,
        "Opéra basé sur l’œuvre source."@fr ;
    rdakit:toolkitLabel "adapted as opera (work)"@en,
        "adaptada como ópera (obra)"@es,
        "adapté en opéra (œuvre)"@fr ;
    reg:hasSubproperty <http://rdaregistry.info/Elements/w/object/P10236> ;
    reg:hasUnconstrained <http://rdaregistry.info/Elements/u/P60722> ;
    reg:lexicalAlias <http://rdaregistry.info/Elements/w/adaptedAsOperaWork.en> ;
    reg:name "adaptedAsOperaWork"@en ;
    reg:status <http://metadataregistry.org/uri/RegStatus/1001> ;
    rdfs:domain <http://rdaregistry.info/Elements/c/C10001> ;
    rdfs:isDefinedBy <http://rdaregistry.info/Elements/w/> ;
    rdfs:subPropertyOf <http://rdaregistry.info/Elements/w/P10155> ;
    skos:definition "Relates a work to an opera based on a source work."@en .

<http://rdaregistry.info/Elements/w/P10247> a rdf:Property ;
    rdfs:label "is choreography (work)"@en ;
    rdakit:instructionNumber "24.5" ;
    rdakit:toolkitDefinition "A work that provides choreography for use in a related work."@en,
        "Una obra que proporciona la coreografía para una obra relacionada."@es,
        "Œuvre qui fournit la chorégraphie destinée à être utilisée dans l’œuvre en relation."@fr ;
    rdakit:toolkitLabel "choreography (work)"@en,
        "coreografía (obra)"@es,
        "chorégraphie (œuvre)"@fr ;
    reg:hasSubproperty <http://rdaregistry.info/Elements/w/object/P10247> ;
    reg:hasUnconstrained <http://rdaregistry.info/Elements/u/P60740> ;
    reg:lexicalAlias <http://rdaregistry.info/Elements/w/choreographyWork.en> ;
    reg:name "choreographyWork"@en ;
    reg:status <http://metadataregistry.org/uri/RegStatus/1001> ;
    rdfs:domain <http://rdaregistry.info/Elements/c/C10001> ;
    rdfs:isDefinedBy <http://rdaregistry.info/Elements/w/> ;
    rdfs:subPropertyOf <http://rdaregistry.info/Elements/w/P10103> ;
    skos:definition "Relates a work to a work that provides choreography for use in a related work."@en .

<http://rdaregistry.info/Elements/w/P10248> a rdf:Property ;
    rdfs:label "is choreography for (work)"@en ;
    rdakit:instructionNumber "24.5" ;
    rdakit:toolkitDefinition "A work that uses choreography of a related work."@en,
        "Una obra que usa la coreografía de una obra relacionada."@es,
        "Œuvre qui utilise la chorégraphie de l’œuvre en relation."@fr ;
    rdakit:toolkitLabel "choreography for (work)"@en,
        "coreografía de (obra)"@es,
        "chorégraphie pour (œuvre)"@fr ;
    reg:hasSubproperty <http://rdaregistry.info/Elements/w/object/P10248> ;
    reg:hasUnconstrained <http://rdaregistry.info/Elements/u/P60741> ;
    reg:lexicalAlias <http://rdaregistry.info/Elements/w/choreographyForWork.en> ;
    reg:name "choreographyForWork"@en ;
    reg:status <http://metadataregistry.org/uri/RegStatus/1001> ;
    rdfs:domain <http://rdaregistry.info/Elements/c/C10001> ;
    rdfs:isDefinedBy <http://rdaregistry.info/Elements/w/> ;
    rdfs:subPropertyOf <http://rdaregistry.info/Elements/w/P10103> ;
    skos:definition "Relates a work to a work that uses choreography of a related work."@en .

<http://rdaregistry.info/Elements/w/P10249> a rdf:Property ;
    rdfs:label "is adapted as video game (work)"@en ;
    rdakit:instructionNumber "24.5" ;
    rdakit:toolkitDefinition "A video game based on a source work."@en,
        "Un video juego basado en la obra fuente."@es,
        "Jeu vidéo basé sur l’œuvre source."@fr ;
    rdakit:toolkitLabel "adapted as video game (work)"@en,
        "adaptada como video juego (obra)"@es,
        "adapté en jeu vidéo (œuvre)"@fr ;
    reg:hasSubproperty <http://rdaregistry.info/Elements/w/object/P10249> ;
    reg:hasUnconstrained <http://rdaregistry.info/Elements/u/P60744> ;
    reg:lexicalAlias <http://rdaregistry.info/Elements/w/adaptedAsVideoGameWork.en> ;
    reg:name "adaptedAsVideoGameWork"@en ;
    reg:status <http://metadataregistry.org/uri/RegStatus/1001> ;
    rdfs:domain <http://rdaregistry.info/Elements/c/C10001> ;
    rdfs:isDefinedBy <http://rdaregistry.info/Elements/w/> ;
    rdfs:subPropertyOf <http://rdaregistry.info/Elements/w/P10155> ;
    skos:definition "Relates a work to a video game based on a source work."@en .

<http://rdaregistry.info/Elements/w/P10250> a rdf:Property ;
    rdfs:label "is video game adaptation of (work)"@en ;
    rdakit:instructionNumber "24.5" ;
    rdakit:toolkitDefinition "A work that has been adapted as a video game."@en,
        "Una obra que ha sido adaptada como un video juego."@es,
        "Œuvre qui a été adaptée en jeu vidéo."@fr ;
    rdakit:toolkitLabel "video game adaptation of (work)"@en,
        "adaptación a video juego de (obra)"@es,
        "adaptation en jeu vidéo de (œuvre)"@fr ;
    reg:hasSubproperty <http://rdaregistry.info/Elements/w/object/P10250> ;
    reg:hasUnconstrained <http://rdaregistry.info/Elements/u/P60745> ;
    reg:lexicalAlias <http://rdaregistry.info/Elements/w/videoGameAdaptationOfWork.en> ;
    reg:name "videoGameAdaptationOfWork"@en ;
    reg:status <http://metadataregistry.org/uri/RegStatus/1001> ;
    rdfs:domain <http://rdaregistry.info/Elements/c/C10001> ;
    rdfs:isDefinedBy <http://rdaregistry.info/Elements/w/> ;
    rdfs:subPropertyOf <http://rdaregistry.info/Elements/w/P10142> ;
    skos:definition "Relates a work to a work that has been adapted as a video game."@en .

<http://rdaregistry.info/Elements/w/P10251> a rdf:Property ;
    rdfs:label "is adapted as graphic novel (work)"@en ;
    rdakit:instructionNumber "24.5" ;
    rdakit:toolkitDefinition "A graphic novel based on a source work."@en,
        "Una novela gráfica basada en la obra fuente"@es,
        "Roman graphique basé sur l’œuvre source."@fr ;
    rdakit:toolkitLabel "adapted as graphic novel (work)"@en,
        "adaptada como novela gráfica (obra)"@es,
        "adapté en roman graphique (œuvre)"@fr ;
    reg:hasSubproperty <http://rdaregistry.info/Elements/w/object/P10251> ;
    reg:hasUnconstrained <http://rdaregistry.info/Elements/u/P60742> ;
    reg:lexicalAlias <http://rdaregistry.info/Elements/w/adaptedAsGraphicNovelWork.en> ;
    reg:name "adaptedAsGraphicNovelWork"@en ;
    reg:status <http://metadataregistry.org/uri/RegStatus/1001> ;
    rdfs:domain <http://rdaregistry.info/Elements/c/C10001> ;
    rdfs:isDefinedBy <http://rdaregistry.info/Elements/w/> ;
    rdfs:subPropertyOf <http://rdaregistry.info/Elements/w/P10155> ;
    skos:definition "Relates a work to a graphic novel based on a source work."@en .

<http://rdaregistry.info/Elements/w/P10252> a rdf:Property ;
    rdfs:label "is graphic novelization of (work)"@en ;
    rdakit:instructionNumber "24.5" ;
    rdakit:toolkitDefinition "A work that has been adapted as a graphic novel."@en,
        "Una obra que ha sido adaptada como una novela gráfica."@es,
        "Œuvre qui a été adaptée en roman graphique."@fr ;
    rdakit:toolkitLabel "graphic novelization of (work)"@en,
        "novelización gráfica de (obra)"@es,
        "adaptation en roman graphique de (œuvre)"@fr ;
    reg:hasSubproperty <http://rdaregistry.info/Elements/w/object/P10252> ;
    reg:hasUnconstrained <http://rdaregistry.info/Elements/u/P60743> ;
    reg:lexicalAlias <http://rdaregistry.info/Elements/w/graphicNovelizationOfWork.en> ;
    reg:name "graphicNovelizationOfWork"@en ;
    reg:status <http://metadataregistry.org/uri/RegStatus/1001> ;
    rdfs:domain <http://rdaregistry.info/Elements/c/C10001> ;
    rdfs:isDefinedBy <http://rdaregistry.info/Elements/w/> ;
    rdfs:subPropertyOf <http://rdaregistry.info/Elements/w/P10142> ;
    skos:definition "Relates a work to a work that has been adapted as a graphic novel."@en .

<http://rdaregistry.info/Elements/w/P10253> a rdf:Property ;
    rdfs:label "has calligrapher"@en ;
    rdakit:instructionNumber "18.5" ;
    rdakit:toolkitDefinition "An artist responsible for creating a work of calligraphy where the focus of interest lies in the aesthetic value of its penmanship or graphic artistry, regardless of whether the same person, etc., also authored the inscribed text."@en,
        "Un artista responsable por la creación de una obra de caligrafía en la cual el foco de interés se centra en el valor estético de su escritura artística o gráfica, independiente de si la misma persona, etc., también es la autora del texto."@es,
        "Artiste responsable de la création d’une œuvre de calligraphie où l’accent est mis sur la valeur esthétique de la calligraphie ou du graphisme, peu importe que la même personne, etc. soit aussi l’auteur du texte calligraphié."@fr ;
    rdakit:toolkitLabel "calligrapher"@en,
        "calígrafo"@es,
        "calligraphe"@fr ;
    reg:hasSubproperty <http://rdaregistry.info/Elements/w/object/P10253> ;
    reg:hasUnconstrained <http://rdaregistry.info/Elements/u/P60752> ;
    reg:lexicalAlias <http://rdaregistry.info/Elements/w/calligrapher.en> ;
    reg:name "calligrapher"@en ;
    reg:status <http://metadataregistry.org/uri/RegStatus/1001> ;
    rdfs:domain <http://rdaregistry.info/Elements/c/C10001> ;
    rdfs:isDefinedBy <http://rdaregistry.info/Elements/w/> ;
    rdfs:subPropertyOf <http://rdaregistry.info/Elements/w/P10058> ;
    skos:definition "Relates a work to an artist responsible for creating a work of calligraphy where the focus of interest lies in the aesthetic value of its penmanship or graphic artistry, regardless of whether the same person, etc., also authored the inscribed text."@en .

<http://rdaregistry.info/Elements/w/P10254> a rdf:Property ;
    rdfs:label "has book artist"@en ;
    rdakit:instructionNumber "18.5" ;
    rdakit:toolkitDefinition "An artist responsible for creating art works that exploit the book form or alter its physical structure as part of the content."@en,
        "Un artista responsable por la creación de obras de arte que aprovechan la forma del libro o alteran su estructura física como parte del contenido de la obra."@es,
        "Artiste responsable de la création d’œuvres d’art qui exploitent la forme livre ou qui modifient sa structure physique comme partie du contenu de l’œuvre."@fr ;
    rdakit:toolkitLabel "book artist"@en,
        "artista del libro"@es,
        "artiste du livre"@fr ;
    reg:hasSubproperty <http://rdaregistry.info/Elements/w/object/P10254> ;
    reg:hasUnconstrained <http://rdaregistry.info/Elements/u/P60753> ;
    reg:lexicalAlias <http://rdaregistry.info/Elements/w/bookArtist.en> ;
    reg:name "bookArtist"@en ;
    reg:status <http://metadataregistry.org/uri/RegStatus/1001> ;
    rdfs:domain <http://rdaregistry.info/Elements/c/C10001> ;
    rdfs:isDefinedBy <http://rdaregistry.info/Elements/w/> ;
    rdfs:subPropertyOf <http://rdaregistry.info/Elements/w/P10058> ;
    skos:definition "Relates a work to an artist responsible for creating art works that exploit the book form or alter its physical structure as part of the content."@en .

<http://rdaregistry.info/Elements/w/P10255> a rdf:Property ;
    rdfs:label "has rapporteur"@en ;
    rdakit:instructionNumber "18.5" ;
    rdakit:seeAlso <http://rdaregistry.info/Elements/e/P20058> ;
    rdakit:toolkitDefinition "An author who is appointed by an organization to report on the proceedings of its meetings."@en,
        "Un autor asignado por una organización para reportar sobre las actas de sus reuniones."@es,
        "Auteur nommé par une organisation pour rédiger les comptes rendus de ses réunions."@fr ;
    rdakit:toolkitLabel "rapporteur"@en,
        "relator"@es,
        "rapporteur"@fr ;
    reg:hasSubproperty <http://rdaregistry.info/Elements/w/object/P10255> ;
    reg:hasUnconstrained <http://rdaregistry.info/Elements/u/P60751> ;
    reg:lexicalAlias <http://rdaregistry.info/Elements/w/rapporteur.en> ;
    reg:name "rapporteur"@en ;
    reg:status <http://metadataregistry.org/uri/RegStatus/1001> ;
    rdfs:domain <http://rdaregistry.info/Elements/c/C10001> ;
    rdfs:isDefinedBy <http://rdaregistry.info/Elements/w/> ;
    rdfs:subPropertyOf <http://rdaregistry.info/Elements/w/P10061> ;
    skos:definition "Relates a work to an author who is appointed by an organization to report on the proceedings of its meetings."@en ;
    skos:scopeNote "Responsibility limited to taking minutes is excluded."@en .

<http://rdaregistry.info/Elements/w/P10266> a rdf:Property ;
    rdfs:label "is analysis of (item)"@en ;
    rdakit:instructionNumber "23.5" ;
    rdakit:toolkitDefinition "An item that has been examined to identify its components and their relations."@en,
        "Un ítem que ha sido examinado para identificar sus componentes y sus relaciones."@es,
        "Item qui a été examiné pour identifier ses composantes et leurs relations."@fr ;
    rdakit:toolkitLabel "analysis of (item)"@en,
        "análisis de (ítem)"@es,
        "analyse de (item)"@fr ;
    reg:hasSubproperty <http://rdaregistry.info/Elements/w/object/P10266> ;
    reg:hasUnconstrained <http://rdaregistry.info/Elements/u/P60239> ;
    reg:lexicalAlias <http://rdaregistry.info/Elements/w/analysisOfItem.en> ;
    reg:name "analysisOfItem"@en ;
    reg:status <http://metadataregistry.org/uri/RegStatus/1001> ;
    rdfs:domain <http://rdaregistry.info/Elements/c/C10001> ;
    rdfs:isDefinedBy <http://rdaregistry.info/Elements/w/> ;
    rdfs:subPropertyOf <http://rdaregistry.info/Elements/w/P10265> ;
    skos:definition "Relates a work to an item that has been examined to identify its components and their relations."@en .

<http://rdaregistry.info/Elements/w/P10267> a rdf:Property ;
    rdfs:label "is evaluation of (item)"@en ;
    rdakit:instructionNumber "23.5" ;
    rdakit:toolkitDefinition "An item that is examined or judged."@en,
        "Un ítem que es examinado o juzgado."@es,
        "Item qui est examiné ou jugé."@fr ;
    rdakit:toolkitLabel "evaluation of (item)"@en,
        "evaluación de (ítem)"@es,
        "évaluation de (item)"@fr ;
    reg:hasSubproperty <http://rdaregistry.info/Elements/w/object/P10267> ;
    reg:hasUnconstrained <http://rdaregistry.info/Elements/u/P60255> ;
    reg:lexicalAlias <http://rdaregistry.info/Elements/w/evaluationOfItem.en> ;
    reg:name "evaluationOfItem"@en ;
    reg:status <http://metadataregistry.org/uri/RegStatus/1001> ;
    rdfs:domain <http://rdaregistry.info/Elements/c/C10001> ;
    rdfs:isDefinedBy <http://rdaregistry.info/Elements/w/> ;
    rdfs:subPropertyOf <http://rdaregistry.info/Elements/w/P10265> ;
    skos:definition "Relates a work to an item that is examined or judged."@en .

<http://rdaregistry.info/Elements/w/P10268> a rdf:Property ;
    rdfs:label "is review of (item)"@en ;
    rdakit:instructionNumber "23.5" ;
    rdakit:toolkitDefinition "An item used as a basis for a brief evaluation."@en,
        "Un ítem usado como base para una evaluación breve."@es,
        "Item servant de base à une brève évaluation."@fr ;
    rdakit:toolkitLabel "review of (item)"@en,
        "reseña de (ítem)"@es,
        "recension de (item)"@fr ;
    reg:hasSubproperty <http://rdaregistry.info/Elements/w/object/P10268> ;
    reg:hasUnconstrained <http://rdaregistry.info/Elements/u/P60288> ;
    reg:lexicalAlias <http://rdaregistry.info/Elements/w/reviewOfItem.en> ;
    reg:name "reviewOfItem"@en ;
    reg:status <http://metadataregistry.org/uri/RegStatus/1001> ;
    rdfs:domain <http://rdaregistry.info/Elements/c/C10001> ;
    rdfs:isDefinedBy <http://rdaregistry.info/Elements/w/> ;
    rdfs:subPropertyOf <http://rdaregistry.info/Elements/w/P10265> ;
    skos:definition "Relates a work to an item used as a basis for a brief evaluation."@en .

<http://rdaregistry.info/Elements/w/P10269> a rdf:Property ;
    rdfs:label "is critique of (item)"@en ;
    rdakit:instructionNumber "23.5" ;
    rdakit:toolkitDefinition "An item used as a basis for a critical evaluation."@en,
        "Un ítem usado como base para una evaluación crítica."@es,
        "Item servant de base à une évaluation critique."@fr ;
    rdakit:toolkitLabel "critique of (item)"@en,
        "crítica de (ítem)"@es,
        "critique de (item)"@fr ;
    reg:hasSubproperty <http://rdaregistry.info/Elements/w/object/P10269> ;
    reg:hasUnconstrained <http://rdaregistry.info/Elements/u/P60292> ;
    reg:lexicalAlias <http://rdaregistry.info/Elements/w/critiqueOfItem.en> ;
    reg:name "critiqueOfItem"@en ;
    reg:status <http://metadataregistry.org/uri/RegStatus/1001> ;
    rdfs:domain <http://rdaregistry.info/Elements/c/C10001> ;
    rdfs:isDefinedBy <http://rdaregistry.info/Elements/w/> ;
    rdfs:subPropertyOf <http://rdaregistry.info/Elements/w/P10265> ;
    skos:definition "Relates a work to an item used as a basis for a critical evaluation."@en .

<http://rdaregistry.info/Elements/w/P10270> a rdf:Property ;
    rdfs:label "is commentary on (item)"@en ;
    rdakit:instructionNumber "23.5" ;
    rdakit:toolkitDefinition "An item used as a basis for a set of explanatory or critical notes."@en,
        "Un ítem usado como base para un conjunto de notas explicativas o críticas."@es,
        "Item servant de base à un ensemble de notes explicatives ou critiques."@fr ;
    rdakit:toolkitLabel "commentary on (item)"@en,
        "comentario sobre (ítem)"@es,
        "commentaire sur (item)"@fr ;
    reg:hasSubproperty <http://rdaregistry.info/Elements/w/object/P10270> ;
    reg:hasUnconstrained <http://rdaregistry.info/Elements/u/P60298> ;
    reg:lexicalAlias <http://rdaregistry.info/Elements/w/commentaryOnItem.en> ;
    reg:name "commentaryOnItem"@en ;
    reg:status <http://metadataregistry.org/uri/RegStatus/1001> ;
    rdfs:domain <http://rdaregistry.info/Elements/c/C10001> ;
    rdfs:isDefinedBy <http://rdaregistry.info/Elements/w/> ;
    rdfs:subPropertyOf <http://rdaregistry.info/Elements/w/P10265> ;
    skos:definition "Relates a work to an item used as a basis for a set of explanatory or critical notes."@en .

<http://rdaregistry.info/Elements/w/P10272> a rdf:Property ;
    rdfs:label "is analysis of (manifestation)"@en ;
    rdakit:instructionNumber "23.5" ;
    rdakit:toolkitDefinition "A manifestation that has been examined to identify its components and their relations."@en,
        "Una manifestación que ha sido examinada para identificar sus componentes y sus relaciones."@es,
        "Manifestation qui a été examinée pour identifier ses composantes et leurs relations."@fr ;
    rdakit:toolkitLabel "analysis of (manifestation)"@en,
        "análisis de (manifestación)"@es,
        "analyse de (manifestation)"@fr ;
    reg:hasSubproperty <http://rdaregistry.info/Elements/w/object/P10272> ;
    reg:hasUnconstrained <http://rdaregistry.info/Elements/u/P60239> ;
    reg:lexicalAlias <http://rdaregistry.info/Elements/w/analysisOfManifestation.en> ;
    reg:name "analysisOfManifestation"@en ;
    reg:status <http://metadataregistry.org/uri/RegStatus/1001> ;
    rdfs:domain <http://rdaregistry.info/Elements/c/C10001> ;
    rdfs:isDefinedBy <http://rdaregistry.info/Elements/w/> ;
    rdfs:subPropertyOf <http://rdaregistry.info/Elements/w/P10271> ;
    skos:definition "Relates a work to a manifestation that has been examined to identify its components and their relations."@en .

<http://rdaregistry.info/Elements/w/P10273> a rdf:Property ;
    rdfs:label "is evaluation of (manifestation)"@en ;
    rdakit:instructionNumber "23.5" ;
    rdakit:toolkitDefinition "A manifestation that is examined or judged."@en,
        "Una manifestación que es examinada o juzgada."@es,
        "Manifestation qui est examinée ou jugée."@fr ;
    rdakit:toolkitLabel "evaluation of (manifestation)"@en,
        "evaluación de (manifestación)"@es,
        "évaluation de (manifestation)"@fr ;
    reg:hasSubproperty <http://rdaregistry.info/Elements/w/object/P10273> ;
    reg:hasUnconstrained <http://rdaregistry.info/Elements/u/P60255> ;
    reg:lexicalAlias <http://rdaregistry.info/Elements/w/evaluationOfManifestation.en> ;
    reg:name "evaluationOfManifestation"@en ;
    reg:status <http://metadataregistry.org/uri/RegStatus/1001> ;
    rdfs:domain <http://rdaregistry.info/Elements/c/C10001> ;
    rdfs:isDefinedBy <http://rdaregistry.info/Elements/w/> ;
    rdfs:subPropertyOf <http://rdaregistry.info/Elements/w/P10271> ;
    skos:definition "Relates a work to a manifestation that is examined or judged."@en .

<http://rdaregistry.info/Elements/w/P10274> a rdf:Property ;
    rdfs:label "is review of (manifestation)"@en ;
    rdakit:instructionNumber "23.5" ;
    rdakit:toolkitDefinition "A manifestation used as a basis for a brief evaluation."@en,
        "Una manifestación usada como base para una evaluacion breve."@es,
        "Manifestation servant de base à une brève évaluation."@fr ;
    rdakit:toolkitLabel "review of (manifestation)"@en,
        "reseña de (manifestación)"@es,
        "recension de (manifestation)"@fr ;
    reg:hasSubproperty <http://rdaregistry.info/Elements/w/object/P10274> ;
    reg:hasUnconstrained <http://rdaregistry.info/Elements/u/P60288> ;
    reg:lexicalAlias <http://rdaregistry.info/Elements/w/reviewOfManifestation.en> ;
    reg:name "reviewOfManifestation"@en ;
    reg:status <http://metadataregistry.org/uri/RegStatus/1001> ;
    rdfs:domain <http://rdaregistry.info/Elements/c/C10001> ;
    rdfs:isDefinedBy <http://rdaregistry.info/Elements/w/> ;
    rdfs:subPropertyOf <http://rdaregistry.info/Elements/w/P10271> ;
    skos:definition "Relates a work to a manifestation used as a basis for a brief evaluation."@en .

<http://rdaregistry.info/Elements/w/P10275> a rdf:Property ;
    rdfs:label "is critique of (manifestation)"@en ;
    rdakit:instructionNumber "23.5" ;
    rdakit:toolkitDefinition "A manifestation used as a basis for a critical evaluation."@en,
        "Una manifestación usada como base para una evaluación crítica."@es,
        "Manifestation servant de base à une évaluation critique."@fr ;
    rdakit:toolkitLabel "critique of (manifestation)"@en,
        "crítica de (manifestación)"@es,
        "critique de (manifestation)"@fr ;
    reg:hasSubproperty <http://rdaregistry.info/Elements/w/object/P10275> ;
    reg:hasUnconstrained <http://rdaregistry.info/Elements/u/P60292> ;
    reg:lexicalAlias <http://rdaregistry.info/Elements/w/critiqueOfManifestation.en> ;
    reg:name "critiqueOfManifestation"@en ;
    reg:status <http://metadataregistry.org/uri/RegStatus/1001> ;
    rdfs:domain <http://rdaregistry.info/Elements/c/C10001> ;
    rdfs:isDefinedBy <http://rdaregistry.info/Elements/w/> ;
    rdfs:subPropertyOf <http://rdaregistry.info/Elements/w/P10271> ;
    skos:definition "Relates a work to a manifestation used as a basis for a critical evaluation."@en .

<http://rdaregistry.info/Elements/w/P10276> a rdf:Property ;
    rdfs:label "is commentary on (manifestation)"@en ;
    rdakit:instructionNumber "23.5" ;
    rdakit:toolkitDefinition "A manifestation used as a basis for a set of explanatory or critical notes."@en,
        "Una manifestación usada como base para un conjunto de notas explicativas o críticas."@es,
        "Manifestation servant de base à un ensemble de notes explicatives ou critiques."@fr ;
    rdakit:toolkitLabel "commentary on (manifestation)"@en,
        "comentario sobre (manifestación)"@es,
        "commentaire sur (manifestation)"@fr ;
    reg:hasSubproperty <http://rdaregistry.info/Elements/w/object/P10276> ;
    reg:hasUnconstrained <http://rdaregistry.info/Elements/u/P60298> ;
    reg:lexicalAlias <http://rdaregistry.info/Elements/w/commentaryOnManifestation.en> ;
    reg:name "commentaryOnManifestation"@en ;
    reg:status <http://metadataregistry.org/uri/RegStatus/1001> ;
    rdfs:domain <http://rdaregistry.info/Elements/c/C10001> ;
    rdfs:isDefinedBy <http://rdaregistry.info/Elements/w/> ;
    rdfs:subPropertyOf <http://rdaregistry.info/Elements/w/P10271> ;
    skos:definition "Relates a work to a manifestation used as a basis for a set of explanatory or critical notes."@en .

<http://rdaregistry.info/Elements/w/P10278> a rdf:Property ;
    rdfs:label "is analysis of (expression)"@en ;
    rdakit:instructionNumber "23.5" ;
    rdakit:toolkitDefinition "An expression that has been examined to identify its components and their relations."@en,
        "Una expresión que ha sido examinada para identificar sus componentes y sus relaciones."@es,
        "Expression qui a été examinée pour identifier ses composantes et leurs relations."@fr ;
    rdakit:toolkitLabel "analysis of (expression)"@en,
        "análisis de (expresión)"@es,
        "analyse de (expression)"@fr ;
    reg:hasSubproperty <http://rdaregistry.info/Elements/w/object/P10278> ;
    reg:hasUnconstrained <http://rdaregistry.info/Elements/u/P60239> ;
    reg:lexicalAlias <http://rdaregistry.info/Elements/w/analysisOfExpression.en> ;
    reg:name "analysisOfExpression"@en ;
    reg:status <http://metadataregistry.org/uri/RegStatus/1001> ;
    rdfs:domain <http://rdaregistry.info/Elements/c/C10001> ;
    rdfs:isDefinedBy <http://rdaregistry.info/Elements/w/> ;
    rdfs:subPropertyOf <http://rdaregistry.info/Elements/w/P10277> ;
    skos:definition "Relates a work to an expression that has been examined to identify its components and their relations."@en .

<http://rdaregistry.info/Elements/w/P10279> a rdf:Property ;
    rdfs:label "is evaluation of (expression)"@en ;
    rdakit:instructionNumber "23.5" ;
    rdakit:toolkitDefinition "An expression that is examined or judged."@en,
        "Una expresión que es examinada o juzgada."@es,
        "Expression qui est examinée ou jugée."@fr ;
    rdakit:toolkitLabel "evaluation of (expression)"@en,
        "evaluación de (expresión)"@es,
        "évaluation de (expression)"@fr ;
    reg:hasSubproperty <http://rdaregistry.info/Elements/w/object/P10279> ;
    reg:hasUnconstrained <http://rdaregistry.info/Elements/u/P60255> ;
    reg:lexicalAlias <http://rdaregistry.info/Elements/w/evaluationOfExpression.en> ;
    reg:name "evaluationOfExpression"@en ;
    reg:status <http://metadataregistry.org/uri/RegStatus/1001> ;
    rdfs:domain <http://rdaregistry.info/Elements/c/C10001> ;
    rdfs:isDefinedBy <http://rdaregistry.info/Elements/w/> ;
    rdfs:subPropertyOf <http://rdaregistry.info/Elements/w/P10277> ;
    skos:definition "Relates a work to an expression that is examined or judged."@en .

<http://rdaregistry.info/Elements/w/P10280> a rdf:Property ;
    rdfs:label "is review of (expression)"@en ;
    rdakit:instructionNumber "23.5" ;
    rdakit:toolkitDefinition "An expression used as a basis for a brief evaluation."@en,
        "Una expresión usada como base para una evaluación breve."@es,
        "Expression servant de base à une brève évaluation."@fr ;
    rdakit:toolkitLabel "review of (expression)"@en,
        "reseña de (expresión)"@es,
        "recension de (expression)"@fr ;
    reg:hasSubproperty <http://rdaregistry.info/Elements/w/object/P10280> ;
    reg:hasUnconstrained <http://rdaregistry.info/Elements/u/P60288> ;
    reg:lexicalAlias <http://rdaregistry.info/Elements/w/reviewOfExpression.en> ;
    reg:name "reviewOfExpression"@en ;
    reg:status <http://metadataregistry.org/uri/RegStatus/1001> ;
    rdfs:domain <http://rdaregistry.info/Elements/c/C10001> ;
    rdfs:isDefinedBy <http://rdaregistry.info/Elements/w/> ;
    rdfs:subPropertyOf <http://rdaregistry.info/Elements/w/P10277> ;
    skos:definition "Relates a work to an expression used as a basis for a brief evaluation."@en .

<http://rdaregistry.info/Elements/w/P10281> a rdf:Property ;
    rdfs:label "is critique of (expression)"@en ;
    rdakit:instructionNumber "23.5" ;
    rdakit:toolkitDefinition "An expression used as a basis for a critical evaluation."@en,
        "Una expresión usada como base para una evaluación crítica."@es,
        "Expression servant de base à une évaluation critique."@fr ;
    rdakit:toolkitLabel "critique of (expression)"@en,
        "crítica de (expresión)"@es,
        "critique de (expression)"@fr ;
    reg:hasSubproperty <http://rdaregistry.info/Elements/w/object/P10281> ;
    reg:hasUnconstrained <http://rdaregistry.info/Elements/u/P60292> ;
    reg:lexicalAlias <http://rdaregistry.info/Elements/w/critiqueOfExpression.en> ;
    reg:name "critiqueOfExpression"@en ;
    reg:status <http://metadataregistry.org/uri/RegStatus/1001> ;
    rdfs:domain <http://rdaregistry.info/Elements/c/C10001> ;
    rdfs:isDefinedBy <http://rdaregistry.info/Elements/w/> ;
    rdfs:subPropertyOf <http://rdaregistry.info/Elements/w/P10277> ;
    skos:definition "Relates a work to an expression used as a basis for a critical evaluation."@en .

<http://rdaregistry.info/Elements/w/P10282> a rdf:Property ;
    rdfs:label "is commentary on (expression)"@en ;
    rdakit:instructionNumber "23.5" ;
    rdakit:toolkitDefinition "An expression used as a basis for a set of explanatory or critical notes."@en,
        "Una expresión usada como base para un conjunto de notas explicativas o críticas."@es,
        "Expression servant de base à un ensemble de notes explicatives ou critiques."@fr ;
    rdakit:toolkitLabel "commentary on (expression)"@en,
        "comentario sobre (expresión)"@es,
        "commentaire sur (expression)"@fr ;
    reg:hasSubproperty <http://rdaregistry.info/Elements/w/object/P10282> ;
    reg:hasUnconstrained <http://rdaregistry.info/Elements/u/P60298> ;
    reg:lexicalAlias <http://rdaregistry.info/Elements/w/commentaryOnExpression.en> ;
    reg:name "commentaryOnexpression"@en ;
    reg:status <http://metadataregistry.org/uri/RegStatus/1001> ;
    rdfs:domain <http://rdaregistry.info/Elements/c/C10001> ;
    rdfs:isDefinedBy <http://rdaregistry.info/Elements/w/> ;
    rdfs:subPropertyOf <http://rdaregistry.info/Elements/w/P10277> ;
    skos:definition "Relates a work to an expression used as a basis for a set of explanatory or critical notes."@en .

<http://rdaregistry.info/Elements/w/P10283> a rdf:Property ;
    rdfs:label "is subject relationship of"@en ;
    rdakit:toolkitDefinition "A work that is about an entity."@en,
        "Una obra que trata sobre la entidad."@es ;
    rdakit:toolkitLabel "subject relationship of"@en,
        "relación de materia de"@es ;
    reg:hasSubproperty <http://rdaregistry.info/Elements/a/object/P50249>,
        <http://rdaregistry.info/Elements/a/object/P50250>,
        <http://rdaregistry.info/Elements/a/object/P50251>,
        <http://rdaregistry.info/Elements/e/P20268>,
        <http://rdaregistry.info/Elements/i/P40061>,
        <http://rdaregistry.info/Elements/m/P30253>,
        <http://rdaregistry.info/Elements/w/P10264>,
        <http://rdaregistry.info/Elements/w/datatype/P10283> ;
    reg:hasUnconstrained <http://rdaregistry.info/Elements/u/P60806> ;
    reg:lexicalAlias <http://rdaregistry.info/Elements/w/SubjectRelationshipOf.en> ;
    reg:name "subjectRelationshipOf"@en ;
    reg:status <http://metadataregistry.org/uri/RegStatus/1001> ;
    rdfs:isDefinedBy <http://rdaregistry.info/Elements/w/> ;
    skos:definition "Relates an entity to a work that is about an entity."@en .

<http://rdaregistry.info/Elements/w/P10284> a rdf:Property ;
    rdfs:label "has degree committee member"@en ;
    rdakit:instructionNumber "18.5" ;
    rdakit:toolkitDefinition "A person serving on a committee that supervises a student's thesis or dissertation."@en,
        "Una persona que sirve en un comité que supervisa una tesis de grado."@es ;
    rdakit:toolkitLabel "degree committee member"@en,
        "miembro del comité de grado"@es ;
    reg:hasSubproperty <http://rdaregistry.info/Elements/w/object/P10284> ;
    reg:hasUnconstrained <http://rdaregistry.info/Elements/u/P60815> ;
    reg:lexicalAlias <http://rdaregistry.info/Elements/w/degreeCommitteeMember.en> ;
    reg:name "degreeCommitteeMember"@en ;
    reg:status <http://metadataregistry.org/uri/RegStatus/1001> ;
    rdfs:domain <http://rdaregistry.info/Elements/c/C10001> ;
    rdfs:isDefinedBy <http://rdaregistry.info/Elements/w/> ;
    rdfs:subPropertyOf <http://rdaregistry.info/Elements/w/P10047> ;
    skos:definition "Relates a work to a person serving on a committee that supervises a student's thesis or dissertation."@en .

<http://rdaregistry.info/Elements/w/P10285> a rdf:Property ;
    rdfs:label "has defendant corporate body"@en ;
    rdakit:instructionNumber "18.5" ;
    rdakit:toolkitDefinition "A corporate body who is accused in a criminal proceeding or sued in a civil proceeding."@en,
        "Una entidad corporativa que es acusada en un proceso penal o demandada en un proceso civil."@es,
        "Collectivité qui est accusée dans une poursuite criminelle ou contre laquelle une poursuite civile est intentée."@fr ;
    rdakit:toolkitLabel "defendant corporate body"@en,
        "entidad corporativa acusada"@es,
        "collectivité défenderesse"@fr ;
    reg:hasSubproperty <http://rdaregistry.info/Elements/w/object/P10285> ;
    reg:hasUnconstrained <http://rdaregistry.info/Elements/u/P60462> ;
    reg:lexicalAlias <http://rdaregistry.info/Elements/w/defendantCorporateBody.en> ;
    reg:name "defendantCorporateBody"@en ;
    reg:status <http://metadataregistry.org/uri/RegStatus/1001> ;
    rdfs:domain <http://rdaregistry.info/Elements/c/C10001> ;
    rdfs:isDefinedBy <http://rdaregistry.info/Elements/w/> ;
    rdfs:subPropertyOf <http://rdaregistry.info/Elements/w/P10040> ;
    skos:definition "Relates a work to a corporate body who is accused in a criminal proceeding or sued in a civil proceeding."@en .

<http://rdaregistry.info/Elements/w/P10286> a rdf:Property ;
    rdfs:label "has defendant person"@en ;
    rdakit:instructionNumber "18.5" ;
    rdakit:toolkitDefinition "A person who is accused in a criminal proceeding or sued in a civil proceeding."@en,
        "Una persona que es acusada en un proceso penal o demandada en un proceso civil."@es,
        "Personne qui est accusée dans une poursuite criminelle ou contre laquelle une poursuite civile est intentée."@fr ;
    rdakit:toolkitLabel "defendant person"@en,
        "persona acusada"@es,
        "personne défenderesse"@fr ;
    reg:hasSubproperty <http://rdaregistry.info/Elements/w/object/P10286> ;
    reg:hasUnconstrained <http://rdaregistry.info/Elements/u/P60462> ;
    reg:lexicalAlias <http://rdaregistry.info/Elements/w/defendantPerson.en> ;
    reg:name "defendantPerson"@en ;
    reg:status <http://metadataregistry.org/uri/RegStatus/1001> ;
    rdfs:domain <http://rdaregistry.info/Elements/c/C10001> ;
    rdfs:isDefinedBy <http://rdaregistry.info/Elements/w/> ;
    rdfs:subPropertyOf <http://rdaregistry.info/Elements/w/P10040> ;
    skos:definition "Relates a work to a person who is accused in a criminal proceeding or sued in a civil proceeding."@en .

<http://rdaregistry.info/Elements/w/P10287> a rdf:Property ;
    rdfs:label "has commissioning body"@en ;
    rdakit:instructionNumber "18.5" ;
    rdakit:toolkitDefinition "An agent responsible for commissioning a work."@en,
        "Una persona, familia o entidad corporativa responsable de la puesta en marcha de una obra."@es ;
    rdakit:toolkitLabel "commissioning body"@en,
        "entidad encargada"@es ;
    reg:hasSubproperty <http://rdaregistry.info/Elements/w/object/P10287> ;
    reg:hasUnconstrained <http://rdaregistry.info/Elements/u/P60826> ;
    reg:lexicalAlias <http://rdaregistry.info/Elements/w/commissioningBody.en> ;
    reg:name "commissioningBody"@en ;
    reg:status <http://metadataregistry.org/uri/RegStatus/1001> ;
    rdfs:domain <http://rdaregistry.info/Elements/c/C10001> ;
    rdfs:isDefinedBy <http://rdaregistry.info/Elements/w/> ;
    rdfs:subPropertyOf <http://rdaregistry.info/Elements/w/P10047> ;
    skos:definition "Relates a work to an agent responsible for commissioning a work."@en .

<http://rdaregistry.info/Elements/w/P10288> a rdf:Property ;
    rdfs:label "is oratorio adaptation of  (work)"@en,
        "is oratorio adaptation of (work)"@en ;
    rdakit:instructionNumber "24.5" ;
    rdakit:toolkitDefinition "A work that has been adapted as an oratorio."@en,
        "Una obra que ha sido adaptada como un oratorio."@es ;
    rdakit:toolkitLabel "oratorio adaptation of (work)"@en,
        "adaptación para oratorio (obra)"@es ;
    reg:hasSubproperty <http://rdaregistry.info/Elements/w/object/P10288> ;
    reg:hasUnconstrained <http://rdaregistry.info/Elements/u/P60830> ;
    reg:lexicalAlias <http://rdaregistry.info/Elements/w/oratorioAdaptationWork.en> ;
    reg:name "oratorioAdaptationOfWork"@en ;
    reg:status <http://metadataregistry.org/uri/RegStatus/1001> ;
    rdfs:domain <http://rdaregistry.info/Elements/c/C10001> ;
    rdfs:isDefinedBy <http://rdaregistry.info/Elements/w/> ;
    rdfs:subPropertyOf <http://rdaregistry.info/Elements/w/P10142> ;
    skos:definition "Relates a work to a work that has been adapted as an oratorio."@en .

<http://rdaregistry.info/Elements/w/P10289> a rdf:Property ;
    rdfs:label "is adapted as oratorio (work)"@en ;
    rdakit:instructionNumber "24.5" ;
    rdakit:toolkitDefinition "An oratorio based on a source work."@en,
        "Un oratorio basado en la obra fuente."@es ;
    rdakit:toolkitLabel "adapted as oratorio (work)"@en,
        "adaptada como oratorio (obra)"@es ;
    reg:hasSubproperty <http://rdaregistry.info/Elements/w/object/P10289> ;
    reg:hasUnconstrained <http://rdaregistry.info/Elements/u/P60831> ;
    reg:lexicalAlias <http://rdaregistry.info/Elements/w/adaptedAsOratorioWork.en> ;
    reg:name "adaptedAsOratorioWork"@en ;
    reg:status <http://metadataregistry.org/uri/RegStatus/1001> ;
    rdfs:domain <http://rdaregistry.info/Elements/c/C10001> ;
    rdfs:isDefinedBy <http://rdaregistry.info/Elements/w/> ;
    rdfs:subPropertyOf <http://rdaregistry.info/Elements/w/P10155> ;
    skos:definition "Relates a work to an oratorio based on a source work."@en .

<http://rdaregistry.info/Elements/w/P10290> a rdf:Property ;
    rdfs:label "is inspired by"@en ;
    rdakit:instructionNumber "24.5" ;
    rdakit:toolkitDefinition "A work which serves as the inspiration for another work."@en,
        "Una obra que sirve de inspiración para otra obra."@es ;
    rdakit:toolkitLabel "inspired by"@en,
        "inspirado por"@es ;
    reg:hasSubproperty <http://rdaregistry.info/Elements/w/object/P10290> ;
    reg:hasUnconstrained <http://rdaregistry.info/Elements/u/P60832> ;
    reg:lexicalAlias <http://rdaregistry.info/Elements/w/inspiredBy.en> ;
    reg:name "inspiredBy"@en ;
    reg:status <http://metadataregistry.org/uri/RegStatus/1001> ;
    rdfs:domain <http://rdaregistry.info/Elements/c/C10001> ;
    rdfs:isDefinedBy <http://rdaregistry.info/Elements/w/> ;
    rdfs:subPropertyOf <http://rdaregistry.info/Elements/w/P10190> ;
    skos:definition "Relates a work to a work which serves as the inspiration for another work."@en .

<http://rdaregistry.info/Elements/w/P10291> a rdf:Property ;
    rdfs:label "is inspiration for"@en ;
    rdakit:instructionNumber "24.5" ;
    rdakit:toolkitDefinition "A work which was inspired by another work."@en,
        "Una obra que se inspira en otra obra."@es ;
    rdakit:toolkitLabel "inspiration for"@en,
        "inspiración para"@es ;
    reg:hasSubproperty <http://rdaregistry.info/Elements/w/object/P10291> ;
    reg:hasUnconstrained <http://rdaregistry.info/Elements/u/P60833> ;
    reg:lexicalAlias <http://rdaregistry.info/Elements/w/inspirationFor.en> ;
    reg:name "inspirationFor"@en ;
    reg:status <http://metadataregistry.org/uri/RegStatus/1001> ;
    rdfs:domain <http://rdaregistry.info/Elements/c/C10001> ;
    rdfs:isDefinedBy <http://rdaregistry.info/Elements/w/> ;
    rdfs:subPropertyOf <http://rdaregistry.info/Elements/w/P10148> ;
    skos:definition "Relates a work to a work which was inspired by another work."@en .

<http://rdaregistry.info/Elements/w/P10292> a rdf:Property ;
    rdfs:label "has participant in treaty"@en ;
    rdakit:instructionNumber "18.5" ;
    rdakit:toolkitDefinition "A government, international intergovernmental body, or other corporate body that has signed, ratified, or acceded to a treaty."@en,
        "Un gobierno, entidad intergubernamental internacional o entidad corporativa que ha firmado, ratificado o accedido a un tratado."@es,
        "Gouvernement, organisation internationale intergouvernementale ou autre collectivité qui a signé ou ratifié un traité ou y a adhéré."@fr ;
    rdakit:toolkitLabel "participant in treaty"@en,
        "participante en un tratado"@es,
        "participant à un traité"@fr ;
    reg:hasSubproperty <http://rdaregistry.info/Elements/w/object/P10292> ;
    reg:hasUnconstrained <http://rdaregistry.info/Elements/u/P60834> ;
    reg:lexicalAlias <http://rdaregistry.info/Elements/w/participantInTreaty.en> ;
    reg:name "participantInTreaty"@en ;
    reg:status <http://metadataregistry.org/uri/RegStatus/1001> ;
    rdfs:domain <http://rdaregistry.info/Elements/c/C10001> ;
    rdfs:isDefinedBy <http://rdaregistry.info/Elements/w/> ;
    rdfs:subPropertyOf <http://rdaregistry.info/Elements/w/P10047> ;
    skos:definition "Relates a work to a government, international intergovernmental body, or other corporate body that has signed, ratified, or acceded to a treaty."@en .

<http://rdaregistry.info/Elements/w/P10293> a rdf:Property ;
    rdfs:label "has researcher"@en ;
    rdakit:instructionNumber "18.5" ;
    rdakit:toolkitDefinition "An agent who does research in support of the creation of a work."@en,
        "Una persona, familia o entidad corporativa que realiza la investigación de apoyo para la creación de una obra."@es ;
    rdakit:toolkitLabel "researcher"@en,
        "investigador"@es ;
    reg:hasSubproperty <http://rdaregistry.info/Elements/w/object/P10293> ;
    reg:hasUnconstrained <http://rdaregistry.info/Elements/u/P60836> ;
    reg:lexicalAlias <http://rdaregistry.info/Elements/w/researcher.en> ;
    reg:name "researcher"@en ;
    reg:status <http://metadataregistry.org/uri/RegStatus/1001> ;
    rdfs:domain <http://rdaregistry.info/Elements/c/C10001> ;
    rdfs:isDefinedBy <http://rdaregistry.info/Elements/w/> ;
    rdfs:subPropertyOf <http://rdaregistry.info/Elements/w/P10047> ;
    skos:definition "Relates a work to an agent who does research in support of the creation of a work."@en .

<http://rdaregistry.info/Elements/w/P10294> a rdf:Property ;
    rdfs:label "has commemoration"@en ;
    rdakit:instructionNumber "24.5" ;
    rdakit:toolkitDefinition "A work created to commemorate an earlier work."@en,
        "Una obra conmemorada por otra obra."@es ;
    rdakit:toolkitLabel "commemoration"@en,
        "conmemoración"@es ;
    reg:hasSubproperty <http://rdaregistry.info/Elements/w/object/P10294> ;
    reg:hasUnconstrained <http://rdaregistry.info/Elements/u/P60846> ;
    reg:lexicalAlias <http://rdaregistry.info/Elements/w/commemoration.en> ;
    reg:name "commemoration"@en ;
    reg:status <http://metadataregistry.org/uri/RegStatus/1001> ;
    rdfs:domain <http://rdaregistry.info/Elements/c/C10001> ;
    rdfs:isDefinedBy <http://rdaregistry.info/Elements/w/> ;
    rdfs:subPropertyOf <http://rdaregistry.info/Elements/w/P10296> ;
    skos:definition "Relates a work to a work created to commemorate a earlier work."@en .

<http://rdaregistry.info/Elements/w/P10295> a rdf:Property ;
    rdfs:label "is commemoration of"@en ;
    rdakit:instructionNumber "24.5" ;
    rdakit:toolkitDefinition "A work commemorated in a later work."@en,
        "Una obra creada para conmemorar otra obra."@es ;
    rdakit:toolkitLabel "commemoration of"@en,
        "conmemoración de"@es ;
    reg:hasSubproperty <http://rdaregistry.info/Elements/w/object/P10295> ;
    reg:hasUnconstrained <http://rdaregistry.info/Elements/u/P60847> ;
    reg:lexicalAlias <http://rdaregistry.info/Elements/w/commemorationOf.en> ;
    reg:name "commemorationOf"@en ;
    reg:status <http://metadataregistry.org/uri/RegStatus/1001> ;
    rdfs:domain <http://rdaregistry.info/Elements/c/C10001> ;
    rdfs:isDefinedBy <http://rdaregistry.info/Elements/w/> ;
    rdfs:subPropertyOf <http://rdaregistry.info/Elements/w/P10296> ;
    skos:definition "Relates a work to a work commemorated in a later work."@en .

<http://rdaregistry.info/Elements/w/P10297> a rdf:Property ;
    rdfs:label "has organizer"@en ;
    rdakit:instructionNumber "18.5" ;
    rdakit:toolkitDefinition "An agent organizing the exhibit, event, conference, course, program, etc., which gave rise to a work."@en,
        "Una persona, familia o entidad corporativa que organiza una exhibición, evento, conferencia, etc., que da origen a una obra."@es,
        "Personne, famille ou collectivité organisant l’exposition, l’événement, le congrès, etc. qui a donné lieu à la création d’une œuvre."@fr ;
    rdakit:toolkitLabel "organizer"@en,
        "organizador"@es,
        "organisateur"@fr ;
    reg:hasSubproperty <http://rdaregistry.info/Elements/w/object/P10297> ;
    reg:hasUnconstrained <http://rdaregistry.info/Elements/u/P60849> ;
    reg:lexicalAlias <http://rdaregistry.info/Elements/w/organizer.en> ;
    reg:name "organizer"@en ;
    reg:status <http://metadataregistry.org/uri/RegStatus/1001> ;
    rdfs:domain <http://rdaregistry.info/Elements/c/C10001> ;
    rdfs:isDefinedBy <http://rdaregistry.info/Elements/w/> ;
    rdfs:subPropertyOf <http://rdaregistry.info/Elements/w/P10047> ;
    skos:definition "Relates a work to an agent organizing the exhibit, event, conference, course, program, etc., which gave rise to a work."@en .

<http://rdaregistry.info/Elements/w/P10298> a rdf:Property ;
    rdfs:label "has editorial director"@en ;
    rdakit:instructionNumber "18.5" ;
    rdakit:seeAlso <http://rdaregistry.info/Elements/e/P20048> ;
    rdakit:toolkitDefinition "An agent having legal and/or intellectual responsibility other than creation for the content of a serial, integrating resource, or multipart monographic work."@en ;
    rdakit:toolkitLabel "editorial director"@en ;
    reg:hasSubproperty <http://rdaregistry.info/Elements/w/object/P10298> ;
    reg:hasUnconstrained <http://rdaregistry.info/Elements/u/P60869> ;
    reg:lexicalAlias <http://rdaregistry.info/Elements/w/editorialDirector.en> ;
    reg:name "editorialDirector"@en ;
    reg:status <http://metadataregistry.org/uri/RegStatus/1001> ;
    rdfs:domain <http://rdaregistry.info/Elements/c/C10001> ;
    rdfs:isDefinedBy <http://rdaregistry.info/Elements/w/> ;
    rdfs:subPropertyOf <http://rdaregistry.info/Elements/w/P10047> ;
    skos:definition "Relates a work to an agent having legal and/or intellectual responsibility other than creation for the content of a serial, integrating resource, or multipart monographic work."@en,
        "Relates a work to an agent having legal or intellectual responsibility other than creation for the content of a serial, integrating resource, or multipart monographic work."@en ;
    skos:scopeNote "Revision, content clarification, etc., in an expression of a work is excluded."@en .

<http://rdaregistry.info/Elements/w/P10299> a rdf:Property ;
    rdfs:label "has founder of work"@en ;
    rdakit:instructionNumber "18.5" ;
    rdakit:toolkitDefinition "An agent responsible for establishing a serial, integrating resource, or multipart monograph."@en ;
    rdakit:toolkitLabel "founder of work"@en ;
    reg:hasSubproperty <http://rdaregistry.info/Elements/w/object/P10299> ;
    reg:hasUnconstrained <http://rdaregistry.info/Elements/u/P60871> ;
    reg:lexicalAlias <http://rdaregistry.info/Elements/w/founderOfWork.en> ;
    reg:name "founderOfWork"@en ;
    reg:status <http://metadataregistry.org/uri/RegStatus/1001> ;
    rdfs:domain <http://rdaregistry.info/Elements/c/C10001> ;
    rdfs:isDefinedBy <http://rdaregistry.info/Elements/w/> ;
    rdfs:subPropertyOf <http://rdaregistry.info/Elements/w/P10047> ;
    skos:definition "Relates a work to an agent responsible for establishing a serial, integrating resource, or multipart monograph."@en .

<http://rdaregistry.info/Elements/w/P10300> a rdf:Property ;
    rdfs:label "has latitude"@en ;
    rdakit:instructionNumber "7.4.2" ;
    rdakit:toolkitDefinition "A distance of a point on a planet or satellite measured north and south from the equator."@en ;
    rdakit:toolkitLabel "latitude"@en ;
    reg:lexicalAlias <http://rdaregistry.info/Elements/w/latitude.en> ;
    reg:name "latitude"@en ;
    reg:status <http://metadataregistry.org/uri/RegStatus/1001> ;
    rdfs:domain <http://rdaregistry.info/Elements/c/C10001> ;
    rdfs:isDefinedBy <http://rdaregistry.info/Elements/w/> ;
    skos:definition "Relates a work to a distance of a point on a planet or satellite measured north and south from the equator."@en .

<http://rdaregistry.info/Elements/w/P10301> a rdf:Property ;
    rdfs:label "has longitude"@en ;
    rdakit:instructionNumber "7.4.2" ;
    rdakit:toolkitDefinition "A distance of a point on a planet or satellite measured east and west from a reference meridian."@en ;
    rdakit:toolkitLabel "longitude"@en ;
    reg:lexicalAlias <http://rdaregistry.info/Elements/w/longitude.en> ;
    reg:name "longitude"@en ;
    reg:status <http://metadataregistry.org/uri/RegStatus/1001> ;
    rdfs:domain <http://rdaregistry.info/Elements/c/C10001> ;
    rdfs:isDefinedBy <http://rdaregistry.info/Elements/w/> ;
    skos:definition "Relates a work to a distance of a point on a planet or satellite measured east and west from a reference meridian."@en .

<http://rdaregistry.info/Elements/w/P10302> a rdf:Property ;
    rdfs:label "has right ascension"@en ;
    rdakit:instructionNumber "7.4.4" ;
    rdakit:toolkitDefinition "An angular distance measured eastward on the equator from the vernal equinox to the hour circle through a celestial body, from 0 to 24 hours."@en ;
    rdakit:toolkitLabel "right ascension"@en ;
    reg:lexicalAlias <http://rdaregistry.info/Elements/w/rightAscension.en> ;
    reg:name "rightAscension"@en ;
    reg:status <http://metadataregistry.org/uri/RegStatus/1001> ;
    rdfs:domain <http://rdaregistry.info/Elements/c/C10001> ;
    rdfs:isDefinedBy <http://rdaregistry.info/Elements/w/> ;
    skos:definition "Relates a work to an angular distance measured eastward on the equator from the vernal equinox to the hour circle through a celestial body, from 0 to 24 hours."@en .

<http://rdaregistry.info/Elements/w/P10303> a rdf:Property ;
    rdfs:label "has declination"@en ;
    rdakit:instructionNumber "7.4.4" ;
    rdakit:toolkitDefinition "An angular distance to a body on the celestial sphere measured north or south through 90° from the celestial equator along the hour circle of the body."@en ;
    rdakit:toolkitLabel "declination"@en ;
    reg:lexicalAlias <http://rdaregistry.info/Elements/w/declination.en> ;
    reg:name "declination"@en ;
    reg:status <http://metadataregistry.org/uri/RegStatus/1001> ;
    rdfs:domain <http://rdaregistry.info/Elements/c/C10001> ;
    rdfs:isDefinedBy <http://rdaregistry.info/Elements/w/> ;
    skos:definition "Relates a work to an angular distance to a body on the celestial sphere measured north or south through 90° from the celestial equator along the hour circle of the body."@en .

<http://rdaregistry.info/Elements/w/P10304> a rdf:Property ;
    rdfs:label "has audio producer"@en ;
    rdakit:instructionNumber "18.5" ;
    rdakit:toolkitDefinition "A producer responsible for most of the business aspects of an audio recording."@en ;
    rdakit:toolkitLabel "audio producer"@en ;
    reg:hasSubproperty <http://rdaregistry.info/Elements/w/object/P10304> ;
    reg:hasUnconstrained <http://rdaregistry.info/Elements/u/P60889> ;
    reg:lexicalAlias <http://rdaregistry.info/Elements/w/audioProducer.en> ;
    reg:name "audioProducer"@en ;
    reg:status <http://metadataregistry.org/uri/RegStatus/1001> ;
    rdfs:domain <http://rdaregistry.info/Elements/c/C10001> ;
    rdfs:isDefinedBy <http://rdaregistry.info/Elements/w/> ;
    rdfs:subPropertyOf <http://rdaregistry.info/Elements/w/P10064> ;
    skos:definition "Relates a work to a producer responsible for most of the business aspects of an audio recording."@en .

<http://rdaregistry.info/Elements/w/P10305> a rdf:Property ;
    rdfs:label "has casting director"@en ;
    rdakit:instructionNumber "18.5" ;
    rdakit:toolkitDefinition "An agent responsible for most aspects of assigning parts and duties to performers."@en ;
    rdakit:toolkitLabel "casting director"@en ;
    reg:hasSubproperty <http://rdaregistry.info/Elements/w/object/P10305> ;
    reg:hasUnconstrained <http://rdaregistry.info/Elements/u/P60890> ;
    reg:lexicalAlias <http://rdaregistry.info/Elements/w/castingDirector.en> ;
    reg:name "castingDirector"@en ;
    reg:status <http://metadataregistry.org/uri/RegStatus/1001> ;
    rdfs:domain <http://rdaregistry.info/Elements/c/C10001> ;
    rdfs:isDefinedBy <http://rdaregistry.info/Elements/w/> ;
    rdfs:subPropertyOf <http://rdaregistry.info/Elements/w/P10047> ;
    skos:definition "Relates a work to an agent responsible for most aspects of assigning parts and duties to performers."@en .

<http://rdaregistry.info/Elements/w/P10306> a rdf:Property ;
    rdfs:label "has remix artist"@en ;
    rdakit:instructionNumber "18.5" ;
    rdakit:seeAlso <http://rdaregistry.info/Elements/e/P20296> ;
    rdakit:toolkitDefinition "An agent responsible for creating an audio work by manipulating, recombining, mixing, and reproducing previously recorded sounds."@en ;
    rdakit:toolkitLabel "remix artist"@en ;
    reg:hasSubproperty <http://rdaregistry.info/Elements/w/object/P10306> ;
    reg:hasUnconstrained <http://rdaregistry.info/Elements/u/P60891> ;
    reg:lexicalAlias <http://rdaregistry.info/Elements/w/remixArtist.en> ;
    reg:name "remixArtist"@en ;
    reg:status <http://metadataregistry.org/uri/RegStatus/1001> ;
    rdfs:domain <http://rdaregistry.info/Elements/c/C10001> ;
    rdfs:isDefinedBy <http://rdaregistry.info/Elements/w/> ;
    rdfs:subPropertyOf <http://rdaregistry.info/Elements/w/P10065> ;
    skos:definition "Relates a work to an agent responsible for creating an audio work by manipulating, recombining, mixing, and reproducing previously recorded sounds."@en ;
    skos:scopeNote "Remixing activities that do not substantially change the nature and content of the original work, and mixing recorded tracks together to appear as one continuous track are excluded."@en .

<http://rdaregistry.info/Elements/w/P10325> a rdf:Property ;
    rdfs:label "is description of (person)"@en ;
    rdakit:instructionNumber "23.5" ;
    rdakit:toolkitDefinition "A person described by a describing work."@en ;
    rdakit:toolkitLabel "description of (person)"@en ;
    reg:hasSubproperty <http://rdaregistry.info/Elements/w/datatype/P10325>,
        <http://rdaregistry.info/Elements/w/object/P10325> ;
    reg:hasUnconstrained <http://rdaregistry.info/Elements/u/P60190> ;
    reg:lexicalAlias <http://rdaregistry.info/Elements/w/descriptionOfPerson.en> ;
    reg:name "descriptionOfPerson"@en ;
    reg:status <http://metadataregistry.org/uri/RegStatus/1001> ;
    rdfs:domain <http://rdaregistry.info/Elements/c/C10001> ;
    rdfs:isDefinedBy <http://rdaregistry.info/Elements/w/> ;
    rdfs:subPropertyOf <http://rdaregistry.info/Elements/w/P10261> ;
    skos:definition "Relates a work to a person described by a describing work."@en .

<http://rdaregistry.info/Elements/w/P10326> a rdf:Property ;
    rdfs:label "is description of (corporate body)"@en ;
    rdakit:instructionNumber "23.5" ;
    rdakit:toolkitDefinition "A corporate body described by a describing work."@en ;
    rdakit:toolkitLabel "description of (corporate body)"@en ;
    reg:hasSubproperty <http://rdaregistry.info/Elements/w/datatype/P10326>,
        <http://rdaregistry.info/Elements/w/object/P10326> ;
    reg:hasUnconstrained <http://rdaregistry.info/Elements/u/P60190> ;
    reg:lexicalAlias <http://rdaregistry.info/Elements/w/descriptionOfCorporateBody.en> ;
    reg:name "descriptionOfCorporateBody"@en ;
    reg:status <http://metadataregistry.org/uri/RegStatus/1001> ;
    rdfs:domain <http://rdaregistry.info/Elements/c/C10001> ;
    rdfs:isDefinedBy <http://rdaregistry.info/Elements/w/> ;
    rdfs:subPropertyOf <http://rdaregistry.info/Elements/w/P10263> ;
    skos:definition "Relates a work to a corporate body described by a describing work."@en .

<http://rdaregistry.info/Elements/w/P10327> a rdf:Property ;
    rdfs:label "is description of (family)"@en ;
    rdakit:instructionNumber "23.5" ;
    rdakit:toolkitDefinition "A family described by a describing work."@en ;
    rdakit:toolkitLabel "description of (family)"@en ;
    reg:hasSubproperty <http://rdaregistry.info/Elements/w/datatype/P10327>,
        <http://rdaregistry.info/Elements/w/object/P10327> ;
    reg:hasUnconstrained <http://rdaregistry.info/Elements/u/P60190> ;
    reg:lexicalAlias <http://rdaregistry.info/Elements/w/descriptionOfFamily.en> ;
    reg:name "descriptionOfFamily"@en ;
    reg:status <http://metadataregistry.org/uri/RegStatus/1001> ;
    rdfs:domain <http://rdaregistry.info/Elements/c/C10001> ;
    rdfs:isDefinedBy <http://rdaregistry.info/Elements/w/> ;
    rdfs:subPropertyOf <http://rdaregistry.info/Elements/w/P10262> ;
    skos:definition "Relates a work to a family described by a describing work."@en .

<http://rdaregistry.info/Elements/w/P10062> a rdf:Property ;
    rdfs:label "has architect"@en ;
    rdakit:instructionNumber "18.5" ;
    rdakit:toolkitDefinition "An agent responsible for creating an architectural design, including a pictorial representation intended to show how a building, etc., will look when completed."@en,
        "Una persona, familia o entidad corporativa responsable de la creación de un diseño arquitectónico, incluyendo una representación pictórica. que muestra como se verá un edificio a su terminación."@es,
        "Personne, famille ou collectivité responsable d’une création architecturale, y compris une représentation illustrée conçue pour montrer de quoi aura l’air un bâtiment, etc. une fois terminé."@fr ;
    rdakit:toolkitLabel "architect"@en,
        "arquitecto"@es,
        "architecte"@fr ;
    reg:hasSubproperty <http://rdaregistry.info/Elements/w/P10200>,
        <http://rdaregistry.info/Elements/w/object/P10062> ;
    reg:hasUnconstrained <http://rdaregistry.info/Elements/u/P60435> ;
    reg:lexicalAlias <http://rdaregistry.info/Elements/w/architect.en> ;
    reg:name "architect"@en ;
    reg:status <http://metadataregistry.org/uri/RegStatus/1001> ;
    rdfs:domain <http://rdaregistry.info/Elements/c/C10001> ;
    rdfs:isDefinedBy <http://rdaregistry.info/Elements/w/> ;
    rdfs:subPropertyOf <http://rdaregistry.info/Elements/w/P10065> ;
    skos:definition "Relates a work to an agent responsible for creating an architectural design, including a pictorial representation intended to show how a building, etc., will look when completed."@en .

<http://rdaregistry.info/Elements/w/P10088> a rdf:Property ;
    rdfs:label "has title of work"@en,
        "har verktitel"@sv ;
    rdakit:instructionNumber "6.2" ;
    rdakit:toolkitDefinition "A word, character, or group of words and/or characters by which a work is known."@en,
        "Una palabra, carácter o grupo de palabras y/o caracteres mediante las cuales se conoce una obra."@es,
        "Mot, caractère ou groupe de mots et/ou de caractères sous lequel une œuvre est connue."@fr ;
    rdakit:toolkitLabel "title of work"@en,
        "título de la obra"@es,
        "titre de l’œuvre"@fr,
        "verktitel"@sv ;
    reg:hasSubproperty <http://rdaregistry.info/Elements/w/P10086>,
        <http://rdaregistry.info/Elements/w/P10223> ;
    reg:hasUnconstrained <http://rdaregistry.info/Elements/u/P60367> ;
    reg:lexicalAlias <http://rdaregistry.info/Elements/w/titleOfWork.en> ;
    reg:name "titleOfWork"@en ;
    reg:status <http://metadataregistry.org/uri/RegStatus/1001> ;
    rdfs:domain <http://rdaregistry.info/Elements/c/C10001> ;
    rdfs:isDefinedBy <http://rdaregistry.info/Elements/w/> ;
    skos:definition "Relates a work to a word, character, or group of words and/or characters by which a work is known."@en .

<http://rdaregistry.info/Elements/w/P10117> a rdf:Property ;
    rdfs:label "is imitated as (work)"@en ;
    rdakit:instructionNumber "24.5" ;
    rdakit:toolkitDefinition "A work that copies the style or content of a source work."@en,
        "Una obra que copia el estilo o contenido de la obra fuente."@es,
        "Œuvre qui copie le style ou le contenu de l’œuvre source."@fr ;
    rdakit:toolkitLabel "imitated as (work)"@en,
        "imitada como (obra)"@es,
        "imité comme (œuvre)"@fr ;
    reg:hasSubproperty <http://rdaregistry.info/Elements/w/P10144>,
        <http://rdaregistry.info/Elements/w/object/P10117> ;
    reg:hasUnconstrained <http://rdaregistry.info/Elements/u/P60214> ;
    reg:lexicalAlias <http://rdaregistry.info/Elements/w/imitatedAsWork.en> ;
    reg:name "imitatedAsWork"@en ;
    reg:status <http://metadataregistry.org/uri/RegStatus/1001> ;
    rdfs:domain <http://rdaregistry.info/Elements/c/C10001> ;
    rdfs:isDefinedBy <http://rdaregistry.info/Elements/w/> ;
    rdfs:subPropertyOf <http://rdaregistry.info/Elements/w/P10148> ;
    skos:definition "Relates a work to a work that copies the style or content of a source work."@en .

<http://rdaregistry.info/Elements/w/P10196> a rdf:Property ;
    rdfs:label "is imitation of (work)"@en ;
    rdakit:instructionNumber "24.5" ;
    rdakit:toolkitDefinition "A work whose style or content is copied in a derivative work."@en,
        "Una obra cuyo estilo o contenido se ha copiado en una obra derivada."@es,
        "Œuvre dont le style ou le contenu est copié dans une œuvre dérivée."@fr ;
    rdakit:toolkitLabel "imitation of (work)"@en,
        "imitación de (obra)"@es,
        "imitation de (œuvre)"@fr ;
    reg:hasSubproperty <http://rdaregistry.info/Elements/w/P10197>,
        <http://rdaregistry.info/Elements/w/object/P10196> ;
    reg:hasUnconstrained <http://rdaregistry.info/Elements/u/P60311> ;
    reg:lexicalAlias <http://rdaregistry.info/Elements/w/imitationOfWork.en> ;
    reg:name "imitationOfWork"@en ;
    reg:status <http://metadataregistry.org/uri/RegStatus/1001> ;
    rdfs:domain <http://rdaregistry.info/Elements/c/C10001> ;
    rdfs:isDefinedBy <http://rdaregistry.info/Elements/w/> ;
    rdfs:subPropertyOf <http://rdaregistry.info/Elements/w/P10190> ;
    skos:definition "Relates a work to a work whose style or content is copied in a derivative work."@en .

<http://rdaregistry.info/Elements/w/P10204> a rdf:Property ;
    rdfs:label "has lyricist"@en ;
    rdakit:instructionNumber "18.5" ;
    rdakit:seeAlso <http://rdaregistry.info/Elements/w/P10205> ;
    rdakit:toolkitDefinition "An author of the words of a popular song, including a song or songs from a musical."@en,
        "Un autor de las palabras de una obra canción popular, incluyendo una canción o canciones de un musical."@es,
        "Auteur des paroles d’une chanson populaire, y compris une ou plusieurs chansons d’une comédie musicale."@fr ;
    rdakit:toolkitLabel "lyricist"@en,
        "letrista"@es,
        "parolier"@fr ;
    reg:hasSubproperty <http://rdaregistry.info/Elements/w/object/P10204> ;
    reg:hasUnconstrained <http://rdaregistry.info/Elements/u/P60477> ;
    reg:lexicalAlias <http://rdaregistry.info/Elements/w/lyricist.en> ;
    reg:name "lyricist"@en ;
    reg:status <http://metadataregistry.org/uri/RegStatus/1001> ;
    rdfs:domain <http://rdaregistry.info/Elements/c/C10001> ;
    rdfs:isDefinedBy <http://rdaregistry.info/Elements/w/> ;
    rdfs:subPropertyOf <http://rdaregistry.info/Elements/w/P10061> ;
    skos:definition "Relates a work to an author of the words of a popular song, including a song or songs from a musical."@en ;
    skos:scopeNote "Authoring of just the dialogue from a musical is excluded"@en .

<http://rdaregistry.info/Elements/w/P10205> a rdf:Property ;
    rdfs:label "has librettist"@en ;
    rdakit:instructionNumber "18.5" ;
    rdakit:seeAlso <http://rdaregistry.info/Elements/w/P10204> ;
    rdakit:toolkitDefinition "An author of the words of an opera or other musical stage work, or an oratorio."@en,
        "Un autor de las palabras de una ópera u otra obra escénica musical, o de un oratorio."@es,
        "Auteur des paroles d’un opéra ou d’une autre œuvre scénique ou d’un oratorio."@fr ;
    rdakit:toolkitLabel "librettist"@en,
        "libretista"@es,
        "librettiste"@fr ;
    reg:hasSubproperty <http://rdaregistry.info/Elements/w/object/P10205> ;
    reg:hasUnconstrained <http://rdaregistry.info/Elements/u/P60478> ;
    reg:lexicalAlias <http://rdaregistry.info/Elements/w/librettist.en> ;
    reg:name "librettist"@en ;
    reg:status <http://metadataregistry.org/uri/RegStatus/1001> ;
    rdfs:domain <http://rdaregistry.info/Elements/c/C10001> ;
    rdfs:isDefinedBy <http://rdaregistry.info/Elements/w/> ;
    rdfs:subPropertyOf <http://rdaregistry.info/Elements/w/P10061> ;
    skos:definition "Relates a work to an author of the words of an opera or other musical stage work, or an oratorio."@en ;
    skos:scopeNote "Authoring of the words of just the songs from a musical is excluded."@en .

<http://rdaregistry.info/Elements/w/P10231> a rdf:Property ;
    rdfs:label "has sequential work relationship with"@en ;
    rdakit:instructionNumber "24.5" ;
    rdakit:toolkitDefinition "A work that is preceded by or succeeded by another work."@en,
        "Una obra que es precedido por o sucedida por la obra."@es,
        "Œuvre qui est précédée ou suivie par l’œuvre."@fr ;
    rdakit:toolkitLabel "sequential work relationship"@en,
        "relaciones de obra secuencial"@es,
        "relation d’œuvre séquentielle"@fr ;
    reg:hasSubproperty <http://rdaregistry.info/Elements/w/P10156>,
        <http://rdaregistry.info/Elements/w/P10170>,
        <http://rdaregistry.info/Elements/w/object/P10231> ;
    reg:hasUnconstrained <http://rdaregistry.info/Elements/u/P60713> ;
    reg:lexicalAlias <http://rdaregistry.info/Elements/w/sequentialWorkRelationship.en> ;
    reg:name "sequentialWorkRelationship"@en ;
    reg:status <http://metadataregistry.org/uri/RegStatus/1001> ;
    rdfs:domain <http://rdaregistry.info/Elements/c/C10001> ;
    rdfs:isDefinedBy <http://rdaregistry.info/Elements/w/> ;
    rdfs:subPropertyOf <http://rdaregistry.info/Elements/w/P10198> ;
    skos:definition "Relates a work to a work that is preceded by or succeeded by another work."@en ;
    skos:scopeNote "Sequential works include sequels, prequels, continuations, superseding works, etc."@en .

<http://rdaregistry.info/Elements/w/P10257> a rdf:Property ;
    rdfs:label "has subject (work)"@en ;
    rdakit:toolkitDefinition "A work that a work is about."@en,
        "Una obra sobre la que trata la obra."@es ;
    rdakit:toolkitLabel "subject (work)"@en,
        "materia (obra)"@es ;
    reg:hasSubproperty <http://rdaregistry.info/Elements/w/datatype/P10257> ;
    reg:hasUnconstrained <http://rdaregistry.info/Elements/u/P60805> ;
    reg:lexicalAlias <http://rdaregistry.info/Elements/w/subjectWork.en> ;
    reg:name "subjectWork"@en ;
    reg:status <http://metadataregistry.org/uri/RegStatus/1001> ;
    rdfs:domain <http://rdaregistry.info/Elements/c/C10001> ;
    rdfs:isDefinedBy <http://rdaregistry.info/Elements/w/> ;
    rdfs:subPropertyOf <http://rdaregistry.info/Elements/w/P10256> ;
    skos:definition "Relates a work to a work that a work is about."@en .

<http://rdaregistry.info/Elements/w/P10258> a rdf:Property ;
    rdfs:label "has subject (expression)"@en ;
    rdakit:toolkitDefinition "An expression that a work is about."@en,
        "Una expresión sobre la que trata la obra."@es ;
    rdakit:toolkitLabel "subject (expression)"@en,
        "materia (expresión)"@es ;
    reg:hasSubproperty <http://rdaregistry.info/Elements/w/P10277>,
        <http://rdaregistry.info/Elements/w/datatype/P10258> ;
    reg:hasUnconstrained <http://rdaregistry.info/Elements/u/P60805> ;
    reg:lexicalAlias <http://rdaregistry.info/Elements/w/subjectExpression.en> ;
    reg:name "subjectExpression"@en ;
    reg:status <http://metadataregistry.org/uri/RegStatus/1001> ;
    rdfs:domain <http://rdaregistry.info/Elements/c/C10001> ;
    rdfs:isDefinedBy <http://rdaregistry.info/Elements/w/> ;
    rdfs:subPropertyOf <http://rdaregistry.info/Elements/w/P10256> ;
    skos:definition "Relates a work to an expression that a work is about."@en .

<http://rdaregistry.info/Elements/w/P10259> a rdf:Property ;
    rdfs:label "has subject (manifestation)"@en ;
    rdakit:toolkitDefinition "A manifestation that a work is about."@en,
        "Una manifestación sobre la que trata la obra."@es ;
    rdakit:toolkitLabel "subject (manifestation)"@en,
        "materia (manifestación)"@es ;
    reg:hasSubproperty <http://rdaregistry.info/Elements/w/P10271>,
        <http://rdaregistry.info/Elements/w/datatype/P10259> ;
    reg:hasUnconstrained <http://rdaregistry.info/Elements/u/P60805> ;
    reg:lexicalAlias <http://rdaregistry.info/Elements/w/subjectManifestation.en> ;
    reg:name "subjectManifestation"@en ;
    reg:status <http://metadataregistry.org/uri/RegStatus/1001> ;
    rdfs:domain <http://rdaregistry.info/Elements/c/C10001> ;
    rdfs:isDefinedBy <http://rdaregistry.info/Elements/w/> ;
    rdfs:subPropertyOf <http://rdaregistry.info/Elements/w/P10256> ;
    skos:definition "Relates a work to a manifestation that a work is about."@en .

<http://rdaregistry.info/Elements/w/P10260> a rdf:Property ;
    rdfs:label "has subject (item)"@en ;
    rdakit:toolkitDefinition "An item that a work is about."@en,
        "Un ítem sobre el que trata la obra."@es ;
    rdakit:toolkitLabel "subject (item)"@en,
        "materia (ítem)"@es ;
    reg:hasSubproperty <http://rdaregistry.info/Elements/w/P10265>,
        <http://rdaregistry.info/Elements/w/datatype/P10260> ;
    reg:hasUnconstrained <http://rdaregistry.info/Elements/u/P60805> ;
    reg:lexicalAlias <http://rdaregistry.info/Elements/w/subjectItem.en> ;
    reg:name "subjectItem"@en ;
    reg:status <http://metadataregistry.org/uri/RegStatus/1001> ;
    rdfs:domain <http://rdaregistry.info/Elements/c/C10001> ;
    rdfs:isDefinedBy <http://rdaregistry.info/Elements/w/> ;
    rdfs:subPropertyOf <http://rdaregistry.info/Elements/w/P10256> ;
    skos:definition "Relates a work to an item that a work is about."@en .

<http://rdaregistry.info/Elements/w/P10261> a rdf:Property ;
    rdfs:label "has subject (person)"@en ;
    rdakit:toolkitDefinition "A person that a work is about."@en,
        "Una persona sobre la que trata la obra."@es ;
    rdakit:toolkitLabel "subject (person)"@en,
        "materia (persona)"@es ;
    reg:hasSubproperty <http://rdaregistry.info/Elements/w/P10325>,
        <http://rdaregistry.info/Elements/w/datatype/P10261> ;
    reg:hasUnconstrained <http://rdaregistry.info/Elements/u/P60805> ;
    reg:lexicalAlias <http://rdaregistry.info/Elements/w/subjectPerson.en> ;
    reg:name "subjectPerson"@en ;
    reg:status <http://metadataregistry.org/uri/RegStatus/1001> ;
    rdfs:domain <http://rdaregistry.info/Elements/c/C10001> ;
    rdfs:isDefinedBy <http://rdaregistry.info/Elements/w/> ;
    rdfs:subPropertyOf <http://rdaregistry.info/Elements/w/P10319> ;
    skos:definition "Relates a work to a person that a work is about."@en .

<http://rdaregistry.info/Elements/w/P10262> a rdf:Property ;
    rdfs:label "has subject (family)"@en ;
    rdakit:toolkitDefinition "A family that a work is about."@en,
        "Una familia sobre la que trata la obra."@es ;
    rdakit:toolkitLabel "subject (family)"@en,
        "materia (familia)"@es ;
    reg:hasSubproperty <http://rdaregistry.info/Elements/w/P10327>,
        <http://rdaregistry.info/Elements/w/datatype/P10262> ;
    reg:hasUnconstrained <http://rdaregistry.info/Elements/u/P60805> ;
    reg:lexicalAlias <http://rdaregistry.info/Elements/w/subjectFamily.en> ;
    reg:name "subjectFamily"@en ;
    reg:status <http://metadataregistry.org/uri/RegStatus/1001> ;
    rdfs:domain <http://rdaregistry.info/Elements/c/C10001> ;
    rdfs:isDefinedBy <http://rdaregistry.info/Elements/w/> ;
    rdfs:subPropertyOf <http://rdaregistry.info/Elements/w/P10320> ;
    skos:definition "Relates a work to a family that a work is about."@en .

<http://rdaregistry.info/Elements/w/P10263> a rdf:Property ;
    rdfs:label "has subject (corporate body)"@en ;
    rdakit:toolkitDefinition "A corporate body that a work is about."@en,
        "Una entidad corporativa sobre la que trata la obra."@es ;
    rdakit:toolkitLabel "subject (corporate body)"@en,
        "materia (entidad corporativa)"@es ;
    reg:hasSubproperty <http://rdaregistry.info/Elements/w/P10326>,
        <http://rdaregistry.info/Elements/w/datatype/P10263> ;
    reg:hasUnconstrained <http://rdaregistry.info/Elements/u/P60805> ;
    reg:lexicalAlias <http://rdaregistry.info/Elements/w/subjectCorporateBody.en> ;
    reg:name "subjectCorporateBody"@en ;
    reg:status <http://metadataregistry.org/uri/RegStatus/1001> ;
    rdfs:domain <http://rdaregistry.info/Elements/c/C10001> ;
    rdfs:isDefinedBy <http://rdaregistry.info/Elements/w/> ;
    rdfs:subPropertyOf <http://rdaregistry.info/Elements/w/P10320> ;
    skos:definition "Relates a work to a corporate body that a work is about."@en .

<http://rdaregistry.info/Elements/w/P10264> a rdf:Property ;
    rdfs:label "is subject of (work)"@en ;
    rdakit:toolkitDefinition "A work that is about a work."@en,
        "Una obra de una obra sobre la que trata la obra."@es ;
    rdakit:toolkitLabel "subject of (work)"@en,
        "materia de (obra)"@es ;
    reg:hasUnconstrained <http://rdaregistry.info/Elements/u/P60806> ;
    reg:lexicalAlias <http://rdaregistry.info/Elements/w/subjectOfWork.en> ;
    reg:name "subjectOfWork"@en ;
    reg:status <http://metadataregistry.org/uri/RegStatus/1001> ;
    rdfs:domain <http://rdaregistry.info/Elements/c/C10001> ;
    rdfs:isDefinedBy <http://rdaregistry.info/Elements/w/> ;
    rdfs:subPropertyOf <http://rdaregistry.info/Elements/w/P10283> ;
    skos:definition "Relates a work to a work that is about a work."@en .

<http://rdaregistry.info/Elements/w/P10315> a rdf:Property ;
    rdfs:label "has related collective agent (work)"@en ;
    reg:hasSubproperty <http://rdaregistry.info/Elements/w/datatype/P10315>,
        <http://rdaregistry.info/Elements/w/object/P10315> ;
    reg:lexicalAlias <http://rdaregistry.info/Elements/w/relatedCollectiveAgentWork.en> ;
    reg:name "relatedCollectiveAgentWork"@en ;
    reg:status <http://metadataregistry.org/uri/RegStatus/1001> ;
    rdfs:domain <http://rdaregistry.info/Elements/c/C10001> ;
    rdfs:isDefinedBy <http://rdaregistry.info/Elements/w/> ;
    rdfs:subPropertyOf <http://rdaregistry.info/Elements/w/P10311> ;
    skos:definition "Relates a work to a collective agent associated with a work being described."@en .

<http://rdaregistry.info/Elements/w/P10319> a rdf:Property ;
    rdfs:label "has subject (agent)"@en ;
    reg:hasUnconstrained <http://rdaregistry.info/Elements/u/P60805> ;
    reg:lexicalAlias <http://rdaregistry.info/Elements/w/subjectAgent.en> ;
    reg:name "subjectAgent"@en ;
    reg:status <http://metadataregistry.org/uri/RegStatus/1001> ;
    rdfs:domain <http://rdaregistry.info/Elements/c/C10001> ;
    rdfs:isDefinedBy <http://rdaregistry.info/Elements/w/> ;
    rdfs:subPropertyOf <http://rdaregistry.info/Elements/w/P10256> ;
    skos:definition "Relates a work to an agent that a work is about."@en .

<http://rdaregistry.info/Elements/w/P10320> a rdf:Property ;
    rdfs:label "has subject (collective agent)"@en ;
    reg:hasUnconstrained <http://rdaregistry.info/Elements/u/P60805> ;
    reg:lexicalAlias <http://rdaregistry.info/Elements/w/subjectCollectiveAgent.en> ;
    reg:name "subjectCollectiveAgent"@en ;
    reg:status <http://metadataregistry.org/uri/RegStatus/1001> ;
    rdfs:domain <http://rdaregistry.info/Elements/c/C10001> ;
    rdfs:isDefinedBy <http://rdaregistry.info/Elements/w/> ;
    rdfs:subPropertyOf <http://rdaregistry.info/Elements/w/P10319> ;
    skos:definition "Relates a work to a collective agent that a work is about."@en .

<http://rdaregistry.info/Elements/w/P10019> a rdf:Property ;
    rdfs:label "is contained in (work)"@en ;
    rdakit:instructionNumber "24.5" ;
    rdakit:toolkitDefinition "A larger work of which a work is a discrete component."@en,
        "Una obra mayor de la cual una parte es un componente separado."@es,
        "Œuvre plus vaste dont l’œuvre est une composante distincte."@fr ;
    rdakit:toolkitLabel "contained in (work)"@en,
        "contenida en (obra)"@es,
        "contenu dans (œuvre)"@fr ;
    reg:hasSubproperty <http://rdaregistry.info/Elements/w/P10101>,
        <http://rdaregistry.info/Elements/w/P10102>,
        <http://rdaregistry.info/Elements/w/object/P10019> ;
    reg:hasUnconstrained <http://rdaregistry.info/Elements/u/P60101> ;
    reg:lexicalAlias <http://rdaregistry.info/Elements/w/containedInWork.en> ;
    reg:name "containedInWork"@en ;
    reg:status <http://metadataregistry.org/uri/RegStatus/1001> ;
    rdfs:domain <http://rdaregistry.info/Elements/c/C10001> ;
    rdfs:isDefinedBy <http://rdaregistry.info/Elements/w/> ;
    rdfs:subPropertyOf <http://rdaregistry.info/Elements/w/P10232> ;
    skos:definition "Relates a work to a larger work of which a work is a discrete component."@en .

<http://rdaregistry.info/Elements/w/P10024> a rdf:Property ;
    rdfs:label "has coordinates of cartographic content"@en,
        "har koordinater (kartografiska resurser)"@sv ;
    rdakit:instructionNumber "7.4" ;
    rdakit:toolkitDefinition "A mathematical system for identifying an area covered by the cartographic content of a work."@en,
        "Un sistema matemático para la identificación del área incluida en el contenido cartográfico de un recurso."@es,
        "Système mathématique servant à identifier la région couverte par le contenu cartographique d’une ressource."@fr ;
    rdakit:toolkitLabel "coordinates of cartographic content"@en,
        "coordenadas del contenido cartográfico"@es,
        "coordonnées d’un contenu cartographique"@fr,
        "koordinater (kartografiska resurser)"@sv ;
    reg:hasSubproperty <http://rdaregistry.info/Elements/w/P10081>,
        <http://rdaregistry.info/Elements/w/P10082>,
        <http://rdaregistry.info/Elements/w/P10083> ;
    reg:hasUnconstrained <http://rdaregistry.info/Elements/u/P60109> ;
    reg:lexicalAlias <http://rdaregistry.info/Elements/w/coordinatesOfCartographicContent.en> ;
    reg:name "coordinatesOfCartographicContent"@en ;
    reg:status <http://metadataregistry.org/uri/RegStatus/1001> ;
    rdfs:domain <http://rdaregistry.info/Elements/c/C10001> ;
    rdfs:isDefinedBy <http://rdaregistry.info/Elements/w/> ;
    skos:definition "Relates a work to a mathematical system for identifying an area covered by the cartographic content of a work."@en ;
    skos:scopeNote "Coordinates may be expressed by means of longitude and latitude on the surface of planets or by the angles of right ascension and declination for celestial charts."@en .

<http://rdaregistry.info/Elements/w/P10037> a rdf:Property ;
    rdfs:label "has appellee"@en ;
    rdakit:instructionNumber "18.5" ;
    rdakit:toolkitDefinition "A person or corporate body against whom an appeal is taken on a decision of a lower court recorded in a legal work of a higher court."@en,
        "Una persona o entidad corporativa contra la cual se hace una apelación sobre una decisión de una corte menor registrada en una obra jurídica de una corte superior."@es,
        "Personne ou collectivité contre laquelle un appel a été formé."@fr ;
    rdakit:toolkitLabel "appellee"@en,
        "apelado"@es,
        "intimé"@fr ;
    reg:hasSubproperty <http://rdaregistry.info/Elements/w/P10005>,
        <http://rdaregistry.info/Elements/w/P10035>,
        <http://rdaregistry.info/Elements/w/datatype/P10037> ;
    reg:hasUnconstrained <http://rdaregistry.info/Elements/u/P60373> ;
    reg:lexicalAlias <http://rdaregistry.info/Elements/w/appellee.en> ;
    reg:name "appellee"@en ;
    reg:status <http://metadataregistry.org/uri/RegStatus/1001> ;
    rdfs:domain <http://rdaregistry.info/Elements/c/C10001> ;
    rdfs:isDefinedBy <http://rdaregistry.info/Elements/w/> ;
    rdfs:subPropertyOf <http://rdaregistry.info/Elements/w/P10047> ;
    skos:definition "Relates a work to a person or corporate body against whom an appeal is taken on a decision of a lower court recorded in a legal work of a higher court."@en .

<http://rdaregistry.info/Elements/w/P10038> a rdf:Property ;
    rdfs:label "has appellant"@en ;
    rdakit:instructionNumber "18.5" ;
    rdakit:toolkitDefinition "A person or corporate body who appeals a decision of a lower court recorded in a legal work of a higher court."@en,
        "Una persona o entidad corporativa que apela una decisión de una corte menor registrada en una obra jurídica de una corte superior."@es,
        "Personne ou collectivité qui en appelle de la décision d’un tribunal inférieur."@fr ;
    rdakit:toolkitLabel "appellant"@en,
        "apelante"@es,
        "appelant"@fr ;
    reg:hasSubproperty <http://rdaregistry.info/Elements/w/P10009>,
        <http://rdaregistry.info/Elements/w/P10042>,
        <http://rdaregistry.info/Elements/w/datatype/P10038> ;
    reg:hasUnconstrained <http://rdaregistry.info/Elements/u/P60457> ;
    reg:lexicalAlias <http://rdaregistry.info/Elements/w/appellant.en> ;
    reg:name "appellant"@en ;
    reg:status <http://metadataregistry.org/uri/RegStatus/1001> ;
    rdfs:domain <http://rdaregistry.info/Elements/c/C10001> ;
    rdfs:isDefinedBy <http://rdaregistry.info/Elements/w/> ;
    rdfs:subPropertyOf <http://rdaregistry.info/Elements/w/P10047> ;
    skos:definition "Relates a work to a person or corporate body who appeals a decision of a lower court recorded in a legal work of a higher court."@en .

<http://rdaregistry.info/Elements/w/P10039> a rdf:Property ;
    rdfs:label "has plaintiff"@en ;
    rdakit:instructionNumber "18.5" ;
    rdakit:toolkitDefinition "A person or corporate body who brings a suit in a civil proceeding."@en,
        "Una persona o entidad corporativa que presenta una demanda en un proceso civil."@es,
        "Personne ou collectivité qui intente une poursuite civile."@fr ;
    rdakit:toolkitLabel "plaintiff"@en,
        "demandante"@es,
        "demandeur"@fr ;
    reg:hasSubproperty <http://rdaregistry.info/Elements/w/P10010>,
        <http://rdaregistry.info/Elements/w/P10043>,
        <http://rdaregistry.info/Elements/w/datatype/P10039> ;
    reg:hasUnconstrained <http://rdaregistry.info/Elements/u/P60459> ;
    reg:lexicalAlias <http://rdaregistry.info/Elements/w/plaintiff.en> ;
    reg:name "plaintiff"@en ;
    reg:status <http://metadataregistry.org/uri/RegStatus/1001> ;
    rdfs:domain <http://rdaregistry.info/Elements/c/C10001> ;
    rdfs:isDefinedBy <http://rdaregistry.info/Elements/w/> ;
    rdfs:subPropertyOf <http://rdaregistry.info/Elements/w/P10047> ;
    skos:definition "Relates a work to a person or corporate body who brings a suit in a civil proceeding."@en .

<http://rdaregistry.info/Elements/w/P10040> a rdf:Property ;
    rdfs:label "has defendant"@en ;
    rdakit:instructionNumber "18.5" ;
    rdakit:toolkitDefinition "A person or corporate body who is accused in a criminal proceeding or sued in a civil proceeding."@en,
        "Una persona o entidad corporativa que es acusada en un proceso penal o demandada en un proceso civil."@es,
        "Personne ou collectivité qui est accusée dans une poursuite criminelle ou contre laquelle une poursuite civile est intentée."@fr ;
    rdakit:toolkitLabel "defendant"@en,
        "acusado"@es,
        "défendeur"@fr ;
    reg:hasSubproperty <http://rdaregistry.info/Elements/w/P10285>,
        <http://rdaregistry.info/Elements/w/P10286>,
        <http://rdaregistry.info/Elements/w/datatype/P10040>,
        <http://rdaregistry.info/Elements/w/object/P10040> ;
    reg:hasUnconstrained <http://rdaregistry.info/Elements/u/P60462> ;
    reg:lexicalAlias <http://rdaregistry.info/Elements/w/defendant.en> ;
    reg:name "defendant"@en ;
    reg:status <http://metadataregistry.org/uri/RegStatus/1001> ;
    rdfs:domain <http://rdaregistry.info/Elements/c/C10001> ;
    rdfs:isDefinedBy <http://rdaregistry.info/Elements/w/> ;
    rdfs:subPropertyOf <http://rdaregistry.info/Elements/w/P10047> ;
    skos:definition "Relates a work to a person or corporate body who is accused in a criminal proceeding or sued in a civil proceeding."@en .

<http://rdaregistry.info/Elements/w/P10147> a rdf:Property ;
    rdfs:label "is container of (work)"@en ;
    rdakit:instructionNumber "24.5" ;
    rdakit:toolkitDefinition "A work that is a discrete component of a larger work."@en,
        "Una obra que es un componente separado de una obra mayor."@es,
        "Œuvre qui est une composante distincte d’une œuvre plus vaste."@fr ;
    rdakit:toolkitLabel "container of (work)"@en,
        "incluye (obra)"@es,
        "conteneur de (œuvre)"@fr ;
    reg:hasSubproperty <http://rdaregistry.info/Elements/w/P10080>,
        <http://rdaregistry.info/Elements/w/P10141>,
        <http://rdaregistry.info/Elements/w/object/P10147> ;
    reg:hasUnconstrained <http://rdaregistry.info/Elements/u/P60249> ;
    reg:lexicalAlias <http://rdaregistry.info/Elements/w/containerOfWork.en> ;
    reg:name "containerOfWork"@en ;
    reg:status <http://metadataregistry.org/uri/RegStatus/1001> ;
    rdfs:domain <http://rdaregistry.info/Elements/c/C10001> ;
    rdfs:isDefinedBy <http://rdaregistry.info/Elements/w/> ;
    rdfs:subPropertyOf <http://rdaregistry.info/Elements/w/P10232> ;
    skos:definition "Relates a work to a work that is a discrete component of a larger work."@en .

<http://rdaregistry.info/Elements/w/P10229> a rdf:Property ;
    rdfs:label "has derivative work relationship with"@en ;
    rdakit:instructionNumber "24.5" ;
    rdakit:toolkitDefinition "A work that is based on or is a derivative of another work."@en,
        "Una obra que se basa en, o es un derivado de la obra."@es,
        "Œuvre qui est basée sur l’œuvre ou en constitue un dérivé."@fr ;
    rdakit:toolkitLabel "derivative work relationship"@en,
        "relaciones de obra derivada"@es,
        "relation d’œuvre dérivée"@fr ;
    reg:hasSubproperty <http://rdaregistry.info/Elements/w/P10148>,
        <http://rdaregistry.info/Elements/w/object/P10229> ;
    reg:hasUnconstrained <http://rdaregistry.info/Elements/u/P60710> ;
    reg:lexicalAlias <http://rdaregistry.info/Elements/w/derivativeWorkRelationship.en> ;
    reg:name "derivativeWorkRelationship"@en ;
    reg:status <http://metadataregistry.org/uri/RegStatus/1001> ;
    rdfs:domain <http://rdaregistry.info/Elements/c/C10001> ;
    rdfs:isDefinedBy <http://rdaregistry.info/Elements/w/> ;
    rdfs:subPropertyOf <http://rdaregistry.info/Elements/w/P10198> ;
    skos:definition "Relates a work to a work that is based on or is a derivative of another work."@en ;
    skos:scopeNote "Derivative works include summaries, abstracts, digests, adaptations, dramatizations, novelizations, screenplays, free translations, paraphrases, imitations, parodies, etc."@en .

<http://rdaregistry.info/Elements/w/P10232> a rdf:Property ;
    rdfs:label "has whole-part work relationship with"@en ;
    rdakit:instructionNumber "24.5" ;
    rdakit:toolkitDefinition "A work that is contained in or contains another work."@en,
        "Una obra que es incluida en, o contiene la obra."@es,
        "Œuvre qui est contenue dans l’œuvre ou la contient."@fr ;
    rdakit:toolkitLabel "whole-part work relationship"@en,
        "relación de la obra todo-parte"@es,
        "relation d’œuvre tout-partie"@fr ;
    reg:hasSubproperty <http://rdaregistry.info/Elements/w/P10019>,
        <http://rdaregistry.info/Elements/w/P10147>,
        <http://rdaregistry.info/Elements/w/object/P10232> ;
    reg:hasUnconstrained <http://rdaregistry.info/Elements/u/P60714> ;
    reg:lexicalAlias <http://rdaregistry.info/Elements/w/wholePartWorkRelationship.en> ;
    reg:name "wholePartWorkRelationship"@en ;
    reg:status <http://metadataregistry.org/uri/RegStatus/1001> ;
    rdfs:domain <http://rdaregistry.info/Elements/c/C10001> ;
    rdfs:isDefinedBy <http://rdaregistry.info/Elements/w/> ;
    rdfs:subPropertyOf <http://rdaregistry.info/Elements/w/P10198> ;
    skos:definition "Relates a work to a work that is contained in or contains another work."@en ;
    skos:scopeNote "Parts of works include discrete components such as subseries, and individual poems, stories, or essays in a collection or anthology."@en .

<http://rdaregistry.info/Elements/w/P10296> a rdf:Property ;
    rdfs:label "has referential work relationship with"@en ;
    rdakit:instructionNumber "24.5" ;
    rdakit:toolkitDefinition "A work that references another work."@en,
        "Una obra que hace referencia a la obra."@es ;
    rdakit:toolkitLabel "referential work relationship"@en,
        "relación obra referencial"@es ;
    reg:hasSubproperty <http://rdaregistry.info/Elements/w/P10294>,
        <http://rdaregistry.info/Elements/w/P10295>,
        <http://rdaregistry.info/Elements/w/object/P10296> ;
    reg:hasUnconstrained <http://rdaregistry.info/Elements/u/P60848> ;
    reg:lexicalAlias <http://rdaregistry.info/Elements/w/referentialWorkRelationship.en> ;
    reg:name "referentialWorkRelationship"@en ;
    reg:status <http://metadataregistry.org/uri/RegStatus/1001> ;
    rdfs:domain <http://rdaregistry.info/Elements/c/C10001> ;
    rdfs:isDefinedBy <http://rdaregistry.info/Elements/w/> ;
    rdfs:subPropertyOf <http://rdaregistry.info/Elements/w/P10198> ;
    skos:definition "Relates a work to a work that references another work."@en .

<http://rdaregistry.info/Elements/w/P10058> a rdf:Property ;
    rdfs:label "has artist"@en ;
    rdakit:instructionNumber "18.5" ;
    rdakit:toolkitDefinition "An agent responsible for creating a work by conceiving, and often implementing, an original graphic design, drawing, painting, etc."@en,
        "Una persona, familia o entidad corporativa responsable de la creación de una obra mediante la concepción, y a menudo la ejecución de un diseño gráfico, un dibujo, una pintura, etc. originales."@es,
        "Personne, famille ou collectivité responsable de la création d’une œuvre par la conception et souvent par la réalisation d’un graphisme, d’une peinture, d’un dessin, etc. original."@fr ;
    rdakit:toolkitLabel "artist"@en,
        "artista"@es,
        "artiste"@fr ;
    reg:hasSubproperty <http://rdaregistry.info/Elements/w/P10202>,
        <http://rdaregistry.info/Elements/w/P10253>,
        <http://rdaregistry.info/Elements/w/P10254>,
        <http://rdaregistry.info/Elements/w/object/P10058> ;
    reg:hasUnconstrained <http://rdaregistry.info/Elements/u/P60431> ;
    reg:lexicalAlias <http://rdaregistry.info/Elements/w/artist.en> ;
    reg:name "artist"@en ;
    reg:status <http://metadataregistry.org/uri/RegStatus/1001> ;
    rdfs:domain <http://rdaregistry.info/Elements/c/C10001> ;
    rdfs:isDefinedBy <http://rdaregistry.info/Elements/w/> ;
    rdfs:subPropertyOf <http://rdaregistry.info/Elements/w/P10065> ;
    skos:definition "Relates a work to an agent responsible for creating a work by conceiving, and often implementing, an original graphic design, drawing, painting, etc."@en .

<http://rdaregistry.info/Elements/w/P10066> a rdf:Property ;
    rdfs:label "has director"@en ;
    rdakit:instructionNumber "18.5" ;
    rdakit:toolkitDefinition "An agent responsible for the general management and supervision of a filmed performance, a radio or television program, etc."@en,
        "Una persona, familia o entidad corporativa responsable de la dirección y supervisión general de una producción cinematográfica, un programa de radio o televisión, etc."@es,
        "Personne, famille ou collectivité responsable de la gestion et de la supervision générales d’une prestation filmée, d’une émission de radio ou de télévision, etc."@fr ;
    rdakit:toolkitLabel "director"@en,
        "director general"@es,
        "réalisateur"@fr ;
    reg:hasSubproperty <http://rdaregistry.info/Elements/w/P10013>,
        <http://rdaregistry.info/Elements/w/P10014>,
        <http://rdaregistry.info/Elements/w/P10015>,
        <http://rdaregistry.info/Elements/w/object/P10066> ;
    reg:hasUnconstrained <http://rdaregistry.info/Elements/u/P60449> ;
    reg:lexicalAlias <http://rdaregistry.info/Elements/w/director.en> ;
    reg:name "director"@en ;
    reg:status <http://metadataregistry.org/uri/RegStatus/1001> ;
    rdfs:domain <http://rdaregistry.info/Elements/c/C10001> ;
    rdfs:isDefinedBy <http://rdaregistry.info/Elements/w/> ;
    rdfs:subPropertyOf <http://rdaregistry.info/Elements/w/P10047> ;
    skos:definition "Relates a work to an agent responsible for the general management and supervision of a filmed performance, a radio or television program, etc."@en .

<http://rdaregistry.info/Elements/w/P10095> a rdf:Property ;
    rdfs:label "is adapted as screenplay (work)"@en ;
    rdakit:instructionNumber "24.5" ;
    rdakit:toolkitDefinition "A work consisting of a screenplay for a motion picture, television program, or video, based on a source work."@en,
        "Una obra que consiste en un guión para una película cinematrográfica, un programa de televisión o video, basado en la obra fuente."@es,
        "Œuvre consistant en le scénario pour un film, une émission de télévision ou une vidéo, basée sur l’œuvre source."@fr ;
    rdakit:toolkitLabel "adapted as screenplay (work)"@en,
        "adaptada como guión (obra)"@es,
        "adapté en scénario (œuvre)"@fr ;
    reg:hasSubproperty <http://rdaregistry.info/Elements/w/P10094>,
        <http://rdaregistry.info/Elements/w/P10096>,
        <http://rdaregistry.info/Elements/w/P10097>,
        <http://rdaregistry.info/Elements/w/object/P10095> ;
    reg:hasUnconstrained <http://rdaregistry.info/Elements/u/P60185> ;
    reg:lexicalAlias <http://rdaregistry.info/Elements/w/adaptedAsScreenplayWork.en> ;
    reg:name "adaptedAsScreenplayWork"@en ;
    reg:status <http://metadataregistry.org/uri/RegStatus/1001> ;
    rdfs:domain <http://rdaregistry.info/Elements/c/C10001> ;
    rdfs:isDefinedBy <http://rdaregistry.info/Elements/w/> ;
    rdfs:subPropertyOf <http://rdaregistry.info/Elements/w/P10155> ;
    skos:definition "Relates a work to a work consisting of a screenplay for a motion picture, television program, or video, based on a source work."@en .

<http://rdaregistry.info/Elements/w/P10105> a rdf:Property ;
    rdfs:label "is screenplay for (work)"@en ;
    rdakit:instructionNumber "24.5" ;
    rdakit:toolkitDefinition "A work such as a motion picture, television program, or video, that uses the text of a work as a screenplay."@en,
        "Una obra tal como una película cinematográfica, programa de televisión o vídeo, que utiliza el texto de la obra como guión."@es,
        "Œuvre telle qu’un film, une émission de télévision ou une vidéo qui utilise le texte de l’œuvre comme scénario."@fr ;
    rdakit:toolkitLabel "screenplay for (work)"@en,
        "guión para (obra)"@es,
        "scénario pour (œuvre)"@fr ;
    reg:hasSubproperty <http://rdaregistry.info/Elements/w/P10173>,
        <http://rdaregistry.info/Elements/w/P10174>,
        <http://rdaregistry.info/Elements/w/P10175>,
        <http://rdaregistry.info/Elements/w/object/P10105> ;
    reg:hasUnconstrained <http://rdaregistry.info/Elements/u/P60201> ;
    reg:lexicalAlias <http://rdaregistry.info/Elements/w/screenplayForWork.en> ;
    reg:name "screenplayForWork"@en ;
    reg:status <http://metadataregistry.org/uri/RegStatus/1001> ;
    rdfs:domain <http://rdaregistry.info/Elements/c/C10001> ;
    rdfs:isDefinedBy <http://rdaregistry.info/Elements/w/> ;
    rdfs:subPropertyOf <http://rdaregistry.info/Elements/w/P10103> ;
    skos:definition "Relates a work to a work such as a motion picture, television program, or video, that uses the text of a work as a screenplay."@en .

<http://rdaregistry.info/Elements/w/P10133> a rdf:Property ;
    rdfs:label "is screenplay based on (work)"@en ;
    rdakit:instructionNumber "24.5" ;
    rdakit:toolkitDefinition "A work that has been adapted as a screenplay for a motion picture, television program, or video."@en,
        "Una obra que ha sido adaptada como guión para una película cinematográfica, programa de televisión o vídeo."@es,
        "Œuvre qui a été adaptée en scénario pour un film, une émission de télévision ou une vidéo."@fr ;
    rdakit:toolkitLabel "screenplay based on (work)"@en,
        "guión basado en (obra)"@es,
        "scénario basé sur (œuvre)"@fr ;
    reg:hasSubproperty <http://rdaregistry.info/Elements/w/P10134>,
        <http://rdaregistry.info/Elements/w/P10135>,
        <http://rdaregistry.info/Elements/w/P10136>,
        <http://rdaregistry.info/Elements/w/object/P10133> ;
    reg:hasUnconstrained <http://rdaregistry.info/Elements/u/P60231> ;
    reg:lexicalAlias <http://rdaregistry.info/Elements/w/screenplayBasedOnWork.en> ;
    reg:name "screenplayBasedOnWork"@en ;
    reg:status <http://metadataregistry.org/uri/RegStatus/1001> ;
    rdfs:domain <http://rdaregistry.info/Elements/c/C10001> ;
    rdfs:isDefinedBy <http://rdaregistry.info/Elements/w/> ;
    rdfs:subPropertyOf <http://rdaregistry.info/Elements/w/P10142> ;
    skos:definition "Relates a work to a work that has been adapted as a screenplay for a motion picture, television program, or video."@en .

<http://rdaregistry.info/Elements/w/P10159> a rdf:Property ;
    rdfs:label "is screenplay (work)"@en ;
    rdakit:instructionNumber "24.5" ;
    rdakit:toolkitDefinition "A work that provides text for a motion picture, television program or video."@en,
        "Una obra que proporciona el texto para una película cinematográfica, programa de televisión o video."@es,
        "Œuvre qui fournit le texte d’un film, d’une émission de télévision ou d’une vidéo."@fr ;
    rdakit:toolkitLabel "screenplay (work)"@en,
        "guión (obra)"@es,
        "scénario (œuvre)"@fr ;
    reg:hasSubproperty <http://rdaregistry.info/Elements/w/P10160>,
        <http://rdaregistry.info/Elements/w/P10163>,
        <http://rdaregistry.info/Elements/w/P10164>,
        <http://rdaregistry.info/Elements/w/object/P10159> ;
    reg:hasUnconstrained <http://rdaregistry.info/Elements/u/P60264> ;
    reg:lexicalAlias <http://rdaregistry.info/Elements/w/screenplayWork.en> ;
    reg:name "screenplayWork"@en ;
    reg:status <http://metadataregistry.org/uri/RegStatus/1001> ;
    rdfs:domain <http://rdaregistry.info/Elements/c/C10001> ;
    rdfs:isDefinedBy <http://rdaregistry.info/Elements/w/> ;
    rdfs:subPropertyOf <http://rdaregistry.info/Elements/w/P10103> ;
    skos:definition "Relates a work to a work that provides text for a motion picture, television program or video."@en .

<http://rdaregistry.info/Elements/w/P10228> a rdf:Property ;
    rdfs:label "has accompanying work relationship with"@en ;
    rdakit:instructionNumber "24.5" ;
    rdakit:toolkitDefinition "A work that is an augmentation of, or is augmented by, or is complemented by another work."@en,
        "Una obra que es un aumento de, o se ve aumentada por, o se complementa con la obra."@es,
        "Œuvre qui constitue une augmentation de l’œuvre ou qui est augmentée ou complétée par elle."@fr ;
    rdakit:toolkitLabel "accompanying work relationship"@en,
        "relaciones de obra acompañante"@es,
        "relation d’œuvre d’accompagnement"@fr ;
    reg:hasSubproperty <http://rdaregistry.info/Elements/w/P10103>,
        <http://rdaregistry.info/Elements/w/P10108>,
        <http://rdaregistry.info/Elements/w/P10192>,
        <http://rdaregistry.info/Elements/w/object/P10228> ;
    reg:hasUnconstrained <http://rdaregistry.info/Elements/u/P60709> ;
    reg:lexicalAlias <http://rdaregistry.info/Elements/w/accompanyingWorkRelationship.en> ;
    reg:name "accompanyingWorkRelationship"@en ;
    reg:status <http://metadataregistry.org/uri/RegStatus/1001> ;
    rdfs:domain <http://rdaregistry.info/Elements/c/C10001> ;
    rdfs:isDefinedBy <http://rdaregistry.info/Elements/w/> ;
    rdfs:subPropertyOf <http://rdaregistry.info/Elements/w/P10198> ;
    skos:definition "Relates a work to a work that is an augmentation of, or is augmented by, or is complemented by another work."@en ;
    skos:scopeNote "Accompanying works include supplements, concordances, indexes, catalogues, teacher’s guides, music for a motion picture, etc."@en .

<http://rdaregistry.info/Elements/w/P10311> a rdf:Property ;
    rdfs:label "has related agent (work)"@en ;
    reg:hasSubproperty <http://rdaregistry.info/Elements/w/datatype/P10311>,
        <http://rdaregistry.info/Elements/w/object/P10311> ;
    reg:lexicalAlias <http://rdaregistry.info/Elements/w/relatedAgentWork.en> ;
    reg:name "relatedAgentWork"@en ;
    reg:status <http://metadataregistry.org/uri/RegStatus/1001> ;
    rdfs:domain <http://rdaregistry.info/Elements/c/C10001> ;
    rdfs:isDefinedBy <http://rdaregistry.info/Elements/w/> ;
    rdfs:subPropertyOf <http://rdaregistry.info/Elements/w/P10307> ;
    skos:definition "Relates a work to an agent associated with a work being described."@en .

<http://rdaregistry.info/Elements/w/P10061> a rdf:Property ;
    rdfs:label "has author"@en ;
    rdakit:instructionNumber "18.5" ;
    rdakit:toolkitDefinition "An agent responsible for creating a work that is primarily textual in content, regardless of media type or genre."@en,
        "Una persona, familia o entidad corporativa responsable de la creación de contenido principalmente textual, independientemente del tipo de medios (por ej., texto impreso, palabra hablada, texto electrónico, texto táctil) o género (por ej., poemas, novelas, guiones, blogs)."@es,
        "Personne, famille ou collectivité responsable de la création d’une œuvre dont le contenu est principalement textuel quel que soit le type de média (par exemple, texte imprimé, parole énoncée, texte électronique, texte tactile) ou le genre (par exemple, poèmes, romans, scénarios, blogues)."@fr ;
    rdakit:toolkitLabel "author"@en,
        "autor"@es,
        "auteur"@fr ;
    reg:hasSubproperty <http://rdaregistry.info/Elements/w/P10203>,
        <http://rdaregistry.info/Elements/w/P10204>,
        <http://rdaregistry.info/Elements/w/P10205>,
        <http://rdaregistry.info/Elements/w/P10255>,
        <http://rdaregistry.info/Elements/w/object/P10061> ;
    reg:hasUnconstrained <http://rdaregistry.info/Elements/u/P60434> ;
    reg:lexicalAlias <http://rdaregistry.info/Elements/w/author.en> ;
    reg:name "author"@en ;
    reg:status <http://metadataregistry.org/uri/RegStatus/1001> ;
    rdfs:domain <http://rdaregistry.info/Elements/c/C10001> ;
    rdfs:isDefinedBy <http://rdaregistry.info/Elements/w/> ;
    rdfs:subPropertyOf <http://rdaregistry.info/Elements/w/P10065> ;
    skos:definition "Relates a work to an agent responsible for creating a work that is primarily textual in content, regardless of media type or genre."@en ;
    skos:scopeNote "Creation of a new work by paraphrasing, rewriting, or adapting works by another creator, if the modification has substantially changed the nature and content of the original or changed the medium of expression, is included."@en .

<http://rdaregistry.info/Elements/w/P10064> a rdf:Property ;
    rdfs:label "has producer"@en ;
    rdakit:instructionNumber "18.5" ;
    rdakit:toolkitDefinition "An agent responsible for most of the business aspects of a production for screen, sound recording, television, webcast, etc."@en,
        "Una persona, familia o entidad corporativa responsable de la mayor parte de los aspectos empresariales de la producción cinematográfica, grabación sonora, televisión, emisión web, etc."@es,
        "Personne, famille ou collectivité responsable de la majeure partie des aspects financiers, techniques et artistiques de la production d’un film, d’un enregistrement audio, d’une émission de télévision, d’une webémission, etc."@fr ;
    rdakit:toolkitLabel "producer"@en,
        "productor"@es,
        "producteur"@fr ;
    reg:hasSubproperty <http://rdaregistry.info/Elements/w/P10073>,
        <http://rdaregistry.info/Elements/w/P10074>,
        <http://rdaregistry.info/Elements/w/P10075>,
        <http://rdaregistry.info/Elements/w/P10304>,
        <http://rdaregistry.info/Elements/w/object/P10064> ;
    reg:hasUnconstrained <http://rdaregistry.info/Elements/u/P60441> ;
    reg:lexicalAlias <http://rdaregistry.info/Elements/w/producer.en> ;
    reg:name "producer"@en ;
    reg:status <http://metadataregistry.org/uri/RegStatus/1001> ;
    rdfs:domain <http://rdaregistry.info/Elements/c/C10001> ;
    rdfs:isDefinedBy <http://rdaregistry.info/Elements/w/> ;
    rdfs:subPropertyOf <http://rdaregistry.info/Elements/w/P10047> ;
    skos:definition "Relates a work to an agent responsible for most of the business aspects of a production for screen, sound recording, television, webcast, etc."@en ;
    skos:scopeNote "The producer is generally responsible for fund raising, managing the production, hiring key personnel, arranging for distributors, etc."@en .

<http://rdaregistry.info/Elements/w/P10198> a rdf:Property ;
    rdfs:label "has related work (work)"@en ;
    reg:hasSubproperty <http://rdaregistry.info/Elements/w/P10228>,
        <http://rdaregistry.info/Elements/w/P10229>,
        <http://rdaregistry.info/Elements/w/P10232>,
        <http://rdaregistry.info/Elements/w/P10296>,
        <http://rdaregistry.info/Elements/w/datatype/P10198>,
        <http://rdaregistry.info/Elements/w/object/P10198> ;
    reg:hasUnconstrained <http://rdaregistry.info/Elements/u/P60313> ;
    reg:lexicalAlias <http://rdaregistry.info/Elements/w/relatedWorkWork.en> ;
    reg:name "relatedWorkWork"@en ;
    reg:status <http://metadataregistry.org/uri/RegStatus/1001> ;
    rdfs:domain <http://rdaregistry.info/Elements/c/C10001> ;
    rdfs:isDefinedBy <http://rdaregistry.info/Elements/w/> ;
    rdfs:subPropertyOf <http://rdaregistry.info/Elements/w/P10307> ;
    skos:definition "Relates a work to a work associated with a work being described."@en .

<http://rdaregistry.info/Elements/w/P10237> a rdf:Property ;
    rdfs:label "is music (work)"@en ;
    rdakit:instructionNumber "24.5" ;
    rdakit:toolkitDefinition "A musical work that is used in a motion picture, play, television program, etc."@en,
        "Una obra musical usada en una película, obra de teatro, programa de televisión, etc."@es,
        "Œuvre musicale utilisée dans un film, une pièce de théâtre, une émission de télévision, etc."@fr ;
    rdakit:toolkitLabel "music (work)"@en,
        "música (obra)"@es,
        "musique (œuvre)"@fr ;
    reg:hasSubproperty <http://rdaregistry.info/Elements/w/P10106>,
        <http://rdaregistry.info/Elements/w/object/P10237> ;
    reg:hasUnconstrained <http://rdaregistry.info/Elements/u/P60723> ;
    reg:lexicalAlias <http://rdaregistry.info/Elements/w/musicWork.en> ;
    reg:name "musicWork"@en ;
    reg:status <http://metadataregistry.org/uri/RegStatus/1001> ;
    rdfs:domain <http://rdaregistry.info/Elements/c/C10001> ;
    rdfs:isDefinedBy <http://rdaregistry.info/Elements/w/> ;
    rdfs:subPropertyOf <http://rdaregistry.info/Elements/w/P10103> ;
    skos:definition "Relates a work to a musical work that is used in a motion picture, play, television program, etc."@en .

<http://rdaregistry.info/Elements/w/P10238> a rdf:Property ;
    rdfs:label "is music for (work)"@en ;
    rdakit:instructionNumber "24.5" ;
    rdakit:toolkitDefinition "A work such as a motion picture, play, television program, etc. that uses a musical work."@en,
        "Una obra tal como una película, obra de teatro, programa de televisión, etc., que usa la obra musical."@es,
        "Œuvre telle qu’un film, une pièce de théâtre, une émission de télévision, etc. qui utilise l’œuvre musicale."@fr ;
    rdakit:toolkitLabel "music for (work)"@en,
        "música para (obra)"@es,
        "musique pour (œuvre)"@fr ;
    reg:hasSubproperty <http://rdaregistry.info/Elements/w/P10031>,
        <http://rdaregistry.info/Elements/w/object/P10238> ;
    reg:hasUnconstrained <http://rdaregistry.info/Elements/u/P60724> ;
    reg:lexicalAlias <http://rdaregistry.info/Elements/w/musicForWork.en> ;
    reg:name "musicForWork"@en ;
    reg:status <http://metadataregistry.org/uri/RegStatus/1001> ;
    rdfs:domain <http://rdaregistry.info/Elements/c/C10001> ;
    rdfs:isDefinedBy <http://rdaregistry.info/Elements/w/> ;
    rdfs:subPropertyOf <http://rdaregistry.info/Elements/w/P10103> ;
    skos:definition "Relates a work to a work such as a motion picture, play, television program, etc., that uses a musical work."@en .

<http://rdaregistry.info/Elements/w/P10100> a rdf:Property ;
    rdfs:label "is description of (work)"@en ;
    rdakit:instructionNumber "23.5" ;
    rdakit:toolkitDefinition "A work described by a describing work."@en,
        "Una obra descrita por una obra que describe."@es,
        "Œuvre décrite par une œuvre descriptive."@fr ;
    rdakit:toolkitLabel "description of (work)"@en,
        "descripción de (obra)"@es,
        "description de (œuvre)"@fr ;
    reg:hasSubproperty <http://rdaregistry.info/Elements/w/P10140>,
        <http://rdaregistry.info/Elements/w/P10153>,
        <http://rdaregistry.info/Elements/w/P10178>,
        <http://rdaregistry.info/Elements/w/P10182>,
        <http://rdaregistry.info/Elements/w/P10187>,
        <http://rdaregistry.info/Elements/w/object/P10100> ;
    reg:hasUnconstrained <http://rdaregistry.info/Elements/u/P60190> ;
    reg:lexicalAlias <http://rdaregistry.info/Elements/w/descriptionOfWork.en> ;
    reg:name "descriptionOfWork"@en ;
    reg:status <http://metadataregistry.org/uri/RegStatus/1001> ;
    rdfs:domain <http://rdaregistry.info/Elements/c/C10001> ;
    rdfs:isDefinedBy <http://rdaregistry.info/Elements/w/> ;
    rdfs:subPropertyOf <http://rdaregistry.info/Elements/w/P10257> ;
    skos:definition "Relates a work to a work described by a describing work."@en .

<http://rdaregistry.info/Elements/w/P10118> a rdf:Property ;
    rdfs:label "is described in (work)"@en ;
    rdakit:instructionNumber "23.5" ;
    rdakit:toolkitDefinition "A work that describes a described work."@en,
        "Una obra que describe una obra descrita."@es,
        "Œuvre qui décrit une œuvre décrite."@fr ;
    rdakit:toolkitLabel "described in (work)"@en,
        "descrita en (obra)"@es,
        "décrit dans (œuvre)"@fr ;
    reg:hasSubproperty <http://rdaregistry.info/Elements/w/P10114>,
        <http://rdaregistry.info/Elements/w/P10115>,
        <http://rdaregistry.info/Elements/w/P10116>,
        <http://rdaregistry.info/Elements/w/P10120>,
        <http://rdaregistry.info/Elements/w/P10121>,
        <http://rdaregistry.info/Elements/w/object/P10118> ;
    reg:hasUnconstrained <http://rdaregistry.info/Elements/u/P60215> ;
    reg:lexicalAlias <http://rdaregistry.info/Elements/w/describedInWork.en> ;
    reg:name "describedInWork"@en ;
    reg:status <http://metadataregistry.org/uri/RegStatus/1001> ;
    rdfs:domain <http://rdaregistry.info/Elements/c/C10001> ;
    rdfs:isDefinedBy <http://rdaregistry.info/Elements/w/> ;
    rdfs:subPropertyOf <http://rdaregistry.info/Elements/w/P10264> ;
    skos:definition "Relates a work to a work that describes a described work."@en .

<http://rdaregistry.info/Elements/w/P10265> a rdf:Property ;
    rdfs:label "is description of (item)"@en ;
    rdakit:instructionNumber "23.5" ;
    rdakit:toolkitDefinition "An item described by a describing work."@en,
        "Un ítem descrito por una obra que describe."@es,
        "Item décrit par une œuvre descriptive."@fr ;
    rdakit:toolkitLabel "description of (item)"@en,
        "descripción de (ítem)"@es,
        "description de (item)"@fr ;
    reg:hasSubproperty <http://rdaregistry.info/Elements/w/P10266>,
        <http://rdaregistry.info/Elements/w/P10267>,
        <http://rdaregistry.info/Elements/w/P10268>,
        <http://rdaregistry.info/Elements/w/P10269>,
        <http://rdaregistry.info/Elements/w/P10270>,
        <http://rdaregistry.info/Elements/w/object/P10265> ;
    reg:hasUnconstrained <http://rdaregistry.info/Elements/u/P60190> ;
    reg:lexicalAlias <http://rdaregistry.info/Elements/w/descriptionOfItem.en> ;
    reg:name "descriptionOfItem"@en ;
    reg:status <http://metadataregistry.org/uri/RegStatus/1001> ;
    rdfs:domain <http://rdaregistry.info/Elements/c/C10001> ;
    rdfs:isDefinedBy <http://rdaregistry.info/Elements/w/> ;
    rdfs:subPropertyOf <http://rdaregistry.info/Elements/w/P10260> ;
    skos:definition "Relates a work to an item described by a describing work."@en .

<http://rdaregistry.info/Elements/w/P10271> a rdf:Property ;
    rdfs:label "is description of (manifestation)"@en ;
    rdakit:instructionNumber "23.5" ;
    rdakit:toolkitDefinition "A manifestation described by a describing work."@en,
        "Una manifestación descrita por una obra que describe."@es,
        "Manifestation décrite par une œuvre descriptive."@fr ;
    rdakit:toolkitLabel "description of (manifestation)"@en,
        "descripción de (manifestación)"@es,
        "description de (manifestation)"@fr ;
    reg:hasSubproperty <http://rdaregistry.info/Elements/w/P10272>,
        <http://rdaregistry.info/Elements/w/P10273>,
        <http://rdaregistry.info/Elements/w/P10274>,
        <http://rdaregistry.info/Elements/w/P10275>,
        <http://rdaregistry.info/Elements/w/P10276>,
        <http://rdaregistry.info/Elements/w/object/P10271> ;
    reg:hasUnconstrained <http://rdaregistry.info/Elements/u/P60190> ;
    reg:lexicalAlias <http://rdaregistry.info/Elements/w/descriptionOfManifestation.en> ;
    reg:name "descriptionOfManifestation"@en ;
    reg:status <http://metadataregistry.org/uri/RegStatus/1001> ;
    rdfs:domain <http://rdaregistry.info/Elements/c/C10001> ;
    rdfs:isDefinedBy <http://rdaregistry.info/Elements/w/> ;
    rdfs:subPropertyOf <http://rdaregistry.info/Elements/w/P10259> ;
    skos:definition "Relates a work to a manifestation described by a describing work."@en .

<http://rdaregistry.info/Elements/w/P10277> a rdf:Property ;
    rdfs:label "is description of (expression)"@en ;
    rdakit:instructionNumber "23.5" ;
    rdakit:toolkitDefinition "An expression described by a describing work."@en,
        "Una expresión descrita por una obra que describe."@es,
        "Expression décrite par une œuvre descriptive."@fr ;
    rdakit:toolkitLabel "description of (expression)"@en,
        "descripción de (expresión)"@es,
        "description de (expression)"@fr ;
    reg:hasSubproperty <http://rdaregistry.info/Elements/w/P10278>,
        <http://rdaregistry.info/Elements/w/P10279>,
        <http://rdaregistry.info/Elements/w/P10280>,
        <http://rdaregistry.info/Elements/w/P10281>,
        <http://rdaregistry.info/Elements/w/P10282>,
        <http://rdaregistry.info/Elements/w/object/P10277> ;
    reg:hasUnconstrained <http://rdaregistry.info/Elements/u/P60190> ;
    reg:lexicalAlias <http://rdaregistry.info/Elements/w/descriptionOfExpression.en> ;
    reg:name "descriptionOfExpression"@en ;
    reg:status <http://metadataregistry.org/uri/RegStatus/1001> ;
    rdfs:domain <http://rdaregistry.info/Elements/c/C10001> ;
    rdfs:isDefinedBy <http://rdaregistry.info/Elements/w/> ;
    rdfs:subPropertyOf <http://rdaregistry.info/Elements/w/P10258> ;
    skos:definition "Relates a work to an expression described by a describing work."@en .

<http://rdaregistry.info/Elements/w/P10256> a rdf:Property ;
    rdfs:label "has subject relationship"@en,
        "har ämnesrelation"@sv ;
    rdakit:instructionNumber "23.5" ;
    rdakit:toolkitDefinition "A relationship between a work and an identifier, an authorized access point, or a description that indicates what a work is about."@en,
        "La relación entre una obra y un identificador, un punto de acceso autorizado y/o una descripción que indica de que trata la obra."@es ;
    rdakit:toolkitLabel "subject relationship"@en,
        "relación de materia"@es,
        "ämnesrelation"@sv ;
    reg:hasSubproperty <http://rdaregistry.info/Elements/w/P10257>,
        <http://rdaregistry.info/Elements/w/P10258>,
        <http://rdaregistry.info/Elements/w/P10259>,
        <http://rdaregistry.info/Elements/w/P10260>,
        <http://rdaregistry.info/Elements/w/P10261>,
        <http://rdaregistry.info/Elements/w/P10262>,
        <http://rdaregistry.info/Elements/w/P10263> ;
    reg:hasUnconstrained <http://rdaregistry.info/Elements/u/P60805> ;
    reg:lexicalAlias <http://rdaregistry.info/Elements/w/subjectRelationship.en> ;
    reg:name "subjectRelationship"@en ;
    reg:status <http://metadataregistry.org/uri/RegStatus/1001> ;
    rdfs:domain <http://rdaregistry.info/Elements/c/C10001> ;
    rdfs:isDefinedBy <http://rdaregistry.info/Elements/w/> ;
    rdfs:subPropertyOf <http://rdaregistry.info/Elements/w/P10307> ;
    skos:definition "Relates a work to a term, phrase, classification number, etc., that indicates what a work is about."@en .

<http://rdaregistry.info/Elements/w/P10307> a rdf:Property ;
    rdfs:label "has related entity (work)"@en ;
    reg:hasSubproperty <http://rdaregistry.info/Elements/w/datatype/P10307>,
        <http://rdaregistry.info/Elements/w/object/P10307> ;
    reg:lexicalAlias <http://rdaregistry.info/Elements/w/relatedEntityWork.en> ;
    reg:name "relatedEntityWork"@en ;
    reg:status <http://metadataregistry.org/uri/RegStatus/1001> ;
    rdfs:domain <http://rdaregistry.info/Elements/c/C10001> ;
    rdfs:isDefinedBy <http://rdaregistry.info/Elements/w/> ;
    rdfs:subPropertyOf <http://rdaregistry.info/Elements/x/P00001> ;
    skos:definition "Relates a work to an entity associated with a work being described."@en .

<http://rdaregistry.info/Elements/w/P10103> a rdf:Property ;
    rdfs:label "is complemented by (work)"@en ;
    rdakit:instructionNumber "24.5" ;
    rdakit:toolkitDefinition "A work paired with another work without either work being considered to predominate."@en,
        "Una obra emparejada con otra sin que ninguna se considere predominante."@es,
        "Œuvre appariée à une autre œuvre sans qu’aucune des deux œuvres ne soit considérée comme prédominante."@fr ;
    rdakit:toolkitLabel "complemented by (work)"@en,
        "complementada por (obra)"@es,
        "complété par (œuvre)"@fr ;
    reg:hasSubproperty <http://rdaregistry.info/Elements/w/P10030>,
        <http://rdaregistry.info/Elements/w/P10105>,
        <http://rdaregistry.info/Elements/w/P10159>,
        <http://rdaregistry.info/Elements/w/P10162>,
        <http://rdaregistry.info/Elements/w/P10165>,
        <http://rdaregistry.info/Elements/w/P10176>,
        <http://rdaregistry.info/Elements/w/P10247>,
        <http://rdaregistry.info/Elements/w/P10248>,
        <http://rdaregistry.info/Elements/w/object/P10103> ;
    reg:hasUnconstrained <http://rdaregistry.info/Elements/u/P60198> ;
    reg:lexicalAlias <http://rdaregistry.info/Elements/w/complementedByWork.en> ;
    reg:name "complementedByWork"@en ;
    reg:status <http://metadataregistry.org/uri/RegStatus/1001> ;
    rdfs:domain <http://rdaregistry.info/Elements/c/C10001> ;
    rdfs:isDefinedBy <http://rdaregistry.info/Elements/w/> ;
    rdfs:subPropertyOf <http://rdaregistry.info/Elements/w/P10228> ;
    skos:definition "Relates a work to a work paired with another work without either work being considered to predominate."@en .

<http://rdaregistry.info/Elements/w/P10156> a rdf:Property ;
    rdfs:label "is preceded by (work)"@en ;
    rdakit:instructionNumber "24.5" ;
    rdakit:toolkitDefinition "A work that precedes, that is, is earlier in time or before in a narrative, etc., a succeeding work."@en,
        "Una obra que precede (por ej., es anterior en el tiempo en una narración) a otra que la sigue."@es,
        "Œuvre qui précède l’œuvre suivante (par exemple, qui lui est antérieure dans le temps ou dans un récit)."@fr ;
    rdakit:toolkitLabel "preceded by (work)"@en,
        "precedida por (obra)"@es,
        "précédé de (œuvre)"@fr ;
    reg:hasSubproperty <http://rdaregistry.info/Elements/w/P10122>,
        <http://rdaregistry.info/Elements/w/P10168>,
        <http://rdaregistry.info/Elements/w/P10169>,
        <http://rdaregistry.info/Elements/w/P10206>,
        <http://rdaregistry.info/Elements/w/P10207>,
        <http://rdaregistry.info/Elements/w/P10213>,
        <http://rdaregistry.info/Elements/w/P10224>,
        <http://rdaregistry.info/Elements/w/P10225>,
        <http://rdaregistry.info/Elements/w/P10226>,
        <http://rdaregistry.info/Elements/w/P10227>,
        <http://rdaregistry.info/Elements/w/object/P10156> ;
    reg:hasUnconstrained <http://rdaregistry.info/Elements/u/P60261> ;
    reg:lexicalAlias <http://rdaregistry.info/Elements/w/precededByWork.en> ;
    reg:name "precededByWork"@en ;
    reg:status <http://metadataregistry.org/uri/RegStatus/1001> ;
    rdfs:domain <http://rdaregistry.info/Elements/c/C10001> ;
    rdfs:isDefinedBy <http://rdaregistry.info/Elements/w/> ;
    rdfs:subPropertyOf <http://rdaregistry.info/Elements/w/P10231> ;
    skos:definition "Relates a work to a work that precedes, that is, is earlier in time or before in a narrative, etc., a succeeding work."@en .

<http://rdaregistry.info/Elements/w/P10170> a rdf:Property ;
    rdfs:label "is succeeded by (work)"@en ;
    rdakit:instructionNumber "24.5" ;
    rdakit:toolkitDefinition "A work that succeeds, that is, is later in time or after in a narrative, etc., a preceding work."@en,
        "Una obra que reemplaza (por ej., más tarde en el tiempo o después en una narración) la obra anterior."@es,
        "Œuvre qui succède à l’œuvre précédente (par exemple, qui lui est ultérieure dans le temps ou dans un récit)."@fr ;
    rdakit:toolkitLabel "succeeded by (work)"@en,
        "reemplazada por (obra)"@es,
        "suivi de (œuvre)"@fr ;
    reg:hasSubproperty <http://rdaregistry.info/Elements/w/P10020>,
        <http://rdaregistry.info/Elements/w/P10021>,
        <http://rdaregistry.info/Elements/w/P10022>,
        <http://rdaregistry.info/Elements/w/P10104>,
        <http://rdaregistry.info/Elements/w/P10145>,
        <http://rdaregistry.info/Elements/w/P10146>,
        <http://rdaregistry.info/Elements/w/P10191>,
        <http://rdaregistry.info/Elements/w/P10195>,
        <http://rdaregistry.info/Elements/w/P10211>,
        <http://rdaregistry.info/Elements/w/P10212>,
        <http://rdaregistry.info/Elements/w/object/P10170> ;
    reg:hasUnconstrained <http://rdaregistry.info/Elements/u/P60278> ;
    reg:lexicalAlias <http://rdaregistry.info/Elements/w/succeededByWork.en> ;
    reg:name "succeededByWork"@en ;
    reg:status <http://metadataregistry.org/uri/RegStatus/1001> ;
    rdfs:domain <http://rdaregistry.info/Elements/c/C10001> ;
    rdfs:isDefinedBy <http://rdaregistry.info/Elements/w/> ;
    rdfs:subPropertyOf <http://rdaregistry.info/Elements/w/P10231> ;
    skos:definition "Relates a work to a work that succeeds, that is, is later in time or after in a narrative, etc., a preceding work."@en .

<http://rdaregistry.info/Elements/w/P10108> a rdf:Property ;
    rdfs:label "is augmented by (work)"@en ;
    rdakit:instructionNumber "24.5" ;
    rdakit:toolkitDefinition "A work that adds to the content of a predominant work."@en,
        "Una obra que agrega al contenido de la obra principal."@es,
        "Œuvre qui ajoute au contenu d’une œuvre prédominante."@fr ;
    rdakit:toolkitLabel "augmented by (work)"@en,
        "ampliada por (obra)"@es,
        "augmenté par (œuvre)"@fr ;
    reg:hasSubproperty <http://rdaregistry.info/Elements/w/P10026>,
        <http://rdaregistry.info/Elements/w/P10092>,
        <http://rdaregistry.info/Elements/w/P10093>,
        <http://rdaregistry.info/Elements/w/P10110>,
        <http://rdaregistry.info/Elements/w/P10111>,
        <http://rdaregistry.info/Elements/w/P10112>,
        <http://rdaregistry.info/Elements/w/P10123>,
        <http://rdaregistry.info/Elements/w/P10124>,
        <http://rdaregistry.info/Elements/w/P10157>,
        <http://rdaregistry.info/Elements/w/P10158>,
        <http://rdaregistry.info/Elements/w/P10172>,
        <http://rdaregistry.info/Elements/w/object/P10108> ;
    reg:hasUnconstrained <http://rdaregistry.info/Elements/u/P60204> ;
    reg:lexicalAlias <http://rdaregistry.info/Elements/w/augmentedByWork.en> ;
    reg:name "augmentedByWork"@en ;
    reg:status <http://metadataregistry.org/uri/RegStatus/1001> ;
    rdfs:domain <http://rdaregistry.info/Elements/c/C10001> ;
    rdfs:isDefinedBy <http://rdaregistry.info/Elements/w/> ;
    rdfs:subPropertyOf <http://rdaregistry.info/Elements/w/P10228> ;
    skos:definition "Relates a work to a work that adds to the content of a predominant work."@en .

<http://rdaregistry.info/Elements/w/P10192> a rdf:Property ;
    rdfs:label "is augmentation of (work)"@en ;
    rdakit:instructionNumber "24.5" ;
    rdakit:toolkitDefinition "A work whose content is added to by another work."@en,
        "Una obra cuyo contenido se agrega a otra obra."@es,
        "Œuvre dont le contenu est accru par une autre œuvre."@fr ;
    rdakit:toolkitLabel "augmentation of (work)"@en,
        "ampliación de (obra)"@es,
        "augmentation de (œuvre)"@fr ;
    reg:hasSubproperty <http://rdaregistry.info/Elements/w/P10029>,
        <http://rdaregistry.info/Elements/w/P10149>,
        <http://rdaregistry.info/Elements/w/P10150>,
        <http://rdaregistry.info/Elements/w/P10151>,
        <http://rdaregistry.info/Elements/w/P10152>,
        <http://rdaregistry.info/Elements/w/P10154>,
        <http://rdaregistry.info/Elements/w/P10177>,
        <http://rdaregistry.info/Elements/w/P10180>,
        <http://rdaregistry.info/Elements/w/P10181>,
        <http://rdaregistry.info/Elements/w/P10188>,
        <http://rdaregistry.info/Elements/w/P10201>,
        <http://rdaregistry.info/Elements/w/object/P10192> ;
    reg:hasUnconstrained <http://rdaregistry.info/Elements/u/P60307> ;
    reg:lexicalAlias <http://rdaregistry.info/Elements/w/augmentationOfWork.en> ;
    reg:name "augmentationOfWork"@en ;
    reg:status <http://metadataregistry.org/uri/RegStatus/1001> ;
    rdfs:domain <http://rdaregistry.info/Elements/c/C10001> ;
    rdfs:isDefinedBy <http://rdaregistry.info/Elements/w/> ;
    rdfs:subPropertyOf <http://rdaregistry.info/Elements/w/P10228> ;
    skos:definition "Relates a work to a work whose content is added to by another work."@en .

<http://rdaregistry.info/Elements/w/P10148> a rdf:Property ;
    rdfs:label "is derivative (work)"@en ;
    rdakit:instructionNumber "24.5" ;
    rdakit:toolkitDefinition "A work that is a modification of a source work."@en,
        "Una obra que es una modificación de una obra fuente."@es,
        "Œuvre qui est une modification d’une œuvre source."@fr ;
    rdakit:toolkitLabel "derivative (work)"@en,
        "obra derivada"@es,
        "dérivé (œuvre)"@fr ;
    reg:hasSubproperty <http://rdaregistry.info/Elements/w/P10028>,
        <http://rdaregistry.info/Elements/w/P10032>,
        <http://rdaregistry.info/Elements/w/P10033>,
        <http://rdaregistry.info/Elements/w/P10089>,
        <http://rdaregistry.info/Elements/w/P10090>,
        <http://rdaregistry.info/Elements/w/P10091>,
        <http://rdaregistry.info/Elements/w/P10099>,
        <http://rdaregistry.info/Elements/w/P10107>,
        <http://rdaregistry.info/Elements/w/P10109>,
        <http://rdaregistry.info/Elements/w/P10113>,
        <http://rdaregistry.info/Elements/w/P10117>,
        <http://rdaregistry.info/Elements/w/P10119>,
        <http://rdaregistry.info/Elements/w/P10155>,
        <http://rdaregistry.info/Elements/w/P10166>,
        <http://rdaregistry.info/Elements/w/P10167>,
        <http://rdaregistry.info/Elements/w/P10171>,
        <http://rdaregistry.info/Elements/w/P10190>,
        <http://rdaregistry.info/Elements/w/P10291>,
        <http://rdaregistry.info/Elements/w/object/P10148> ;
    reg:hasUnconstrained <http://rdaregistry.info/Elements/u/P60250> ;
    reg:lexicalAlias <http://rdaregistry.info/Elements/w/derivativeWork.en> ;
    reg:name "derivativeWork"@en ;
    reg:status <http://metadataregistry.org/uri/RegStatus/1001> ;
    rdfs:domain <http://rdaregistry.info/Elements/c/C10001> ;
    rdfs:isDefinedBy <http://rdaregistry.info/Elements/w/> ;
    rdfs:subPropertyOf <http://rdaregistry.info/Elements/w/P10229> ;
    skos:definition "Relates a work to a work that is a modification of a source work."@en .

<http://rdaregistry.info/Elements/w/P10190> a rdf:Property ;
    rdfs:label "is based on (work)"@en ;
    rdakit:instructionNumber "24.5" ;
    rdakit:toolkitDefinition "A work used as a source for a derivative work."@en,
        "Una obra utilizada como fuente para una obra derivada."@es,
        "Œuvre servant de source à une œuvre dérivée."@fr ;
    rdakit:toolkitLabel "based on (work)"@en,
        "basada en (obra)"@es,
        "basé sur (œuvre)"@fr ;
    reg:hasSubproperty <http://rdaregistry.info/Elements/w/P10027>,
        <http://rdaregistry.info/Elements/w/P10125>,
        <http://rdaregistry.info/Elements/w/P10126>,
        <http://rdaregistry.info/Elements/w/P10139>,
        <http://rdaregistry.info/Elements/w/P10142>,
        <http://rdaregistry.info/Elements/w/P10143>,
        <http://rdaregistry.info/Elements/w/P10161>,
        <http://rdaregistry.info/Elements/w/P10179>,
        <http://rdaregistry.info/Elements/w/P10183>,
        <http://rdaregistry.info/Elements/w/P10184>,
        <http://rdaregistry.info/Elements/w/P10185>,
        <http://rdaregistry.info/Elements/w/P10186>,
        <http://rdaregistry.info/Elements/w/P10189>,
        <http://rdaregistry.info/Elements/w/P10193>,
        <http://rdaregistry.info/Elements/w/P10194>,
        <http://rdaregistry.info/Elements/w/P10196>,
        <http://rdaregistry.info/Elements/w/P10290>,
        <http://rdaregistry.info/Elements/w/object/P10190> ;
    reg:hasUnconstrained <http://rdaregistry.info/Elements/u/P60305> ;
    reg:lexicalAlias <http://rdaregistry.info/Elements/w/basedOnWork.en> ;
    reg:name "basedOnWork"@en ;
    reg:status <http://metadataregistry.org/uri/RegStatus/1001> ;
    rdfs:domain <http://rdaregistry.info/Elements/c/C10001> ;
    rdfs:isDefinedBy <http://rdaregistry.info/Elements/w/> ;
    rdfs:subPropertyOf <http://rdaregistry.info/Elements/w/P10229> ;
    skos:definition "Relates a work to a work used as a source for a derivative work."@en .

<http://rdaregistry.info/Elements/w/P10142> a rdf:Property ;
    rdfs:label "is adaptation of (work)"@en ;
    rdakit:instructionNumber "24.5" ;
    rdakit:toolkitDefinition "A work that has been modified for a purpose, use, or medium other than that for which it was originally intended."@en,
        "Una obra que ha sido modificada para un propósito, uso o medio diferente de los previstos originalmente."@es,
        "Œuvre qui a été modifiée pour une fin, une utilisation ou un mode d’expression autre que celui auquel elle était destinée à l’origine."@fr ;
    rdakit:toolkitLabel "adaptation of (work)"@en,
        "adaptación de (obra)"@es,
        "adaptation de (œuvre)"@fr ;
    reg:hasSubproperty <http://rdaregistry.info/Elements/w/P10127>,
        <http://rdaregistry.info/Elements/w/P10128>,
        <http://rdaregistry.info/Elements/w/P10129>,
        <http://rdaregistry.info/Elements/w/P10130>,
        <http://rdaregistry.info/Elements/w/P10131>,
        <http://rdaregistry.info/Elements/w/P10132>,
        <http://rdaregistry.info/Elements/w/P10133>,
        <http://rdaregistry.info/Elements/w/P10137>,
        <http://rdaregistry.info/Elements/w/P10138>,
        <http://rdaregistry.info/Elements/w/P10233>,
        <http://rdaregistry.info/Elements/w/P10234>,
        <http://rdaregistry.info/Elements/w/P10250>,
        <http://rdaregistry.info/Elements/w/P10252>,
        <http://rdaregistry.info/Elements/w/P10288>,
        <http://rdaregistry.info/Elements/w/object/P10142> ;
    reg:hasUnconstrained <http://rdaregistry.info/Elements/u/P60241> ;
    reg:lexicalAlias <http://rdaregistry.info/Elements/w/adaptationOfWork.en> ;
    reg:name "adaptationOfWork"@en ;
    reg:status <http://metadataregistry.org/uri/RegStatus/1001> ;
    rdfs:domain <http://rdaregistry.info/Elements/c/C10001> ;
    rdfs:isDefinedBy <http://rdaregistry.info/Elements/w/> ;
    rdfs:subPropertyOf <http://rdaregistry.info/Elements/w/P10190> ;
    skos:definition "Relates a work to a work that has been modified for a purpose, use, or medium other than that for which it was originally intended."@en ;
    skos:scopeNote "This relationship applies to changes in form or to works completely rewritten in the same form."@en .

<http://rdaregistry.info/Elements/w/P10155> a rdf:Property ;
    rdfs:label "is adapted as (work)"@en ;
    rdakit:instructionNumber "24.5" ;
    rdakit:toolkitDefinition "A work that modifies a source work for a purpose, use, or medium other than that for which it was originally intended."@en,
        "Una obra que modifica la obra fuente para un propósito, uso o medio diferente del previsto originalmente."@es,
        "Œuvre qui modifie l’œuvre source pour une fin, une utilisation ou un mode d’expression autre que celui auquel elle était destinée à l’origine."@fr ;
    rdakit:toolkitLabel "adapted as (work)"@en,
        "adaptada como (obra)"@es,
        "adapté comme (œuvre)"@fr ;
    reg:hasSubproperty <http://rdaregistry.info/Elements/w/P10016>,
        <http://rdaregistry.info/Elements/w/P10023>,
        <http://rdaregistry.info/Elements/w/P10025>,
        <http://rdaregistry.info/Elements/w/P10034>,
        <http://rdaregistry.info/Elements/w/P10076>,
        <http://rdaregistry.info/Elements/w/P10085>,
        <http://rdaregistry.info/Elements/w/P10087>,
        <http://rdaregistry.info/Elements/w/P10095>,
        <http://rdaregistry.info/Elements/w/P10098>,
        <http://rdaregistry.info/Elements/w/P10235>,
        <http://rdaregistry.info/Elements/w/P10236>,
        <http://rdaregistry.info/Elements/w/P10249>,
        <http://rdaregistry.info/Elements/w/P10251>,
        <http://rdaregistry.info/Elements/w/P10289>,
        <http://rdaregistry.info/Elements/w/object/P10155> ;
    reg:hasUnconstrained <http://rdaregistry.info/Elements/u/P60260> ;
    reg:lexicalAlias <http://rdaregistry.info/Elements/w/adaptedAsWork.en> ;
    reg:name "adaptedAsWork"@en ;
    reg:status <http://metadataregistry.org/uri/RegStatus/1001> ;
    rdfs:domain <http://rdaregistry.info/Elements/c/C10001> ;
    rdfs:isDefinedBy <http://rdaregistry.info/Elements/w/> ;
    rdfs:subPropertyOf <http://rdaregistry.info/Elements/w/P10148> ;
    skos:definition "Relates a work to a work that modifies a source work for a purpose, use, or medium other than that for which it was originally intended."@en ;
    skos:scopeNote "This relationship applies to changes in form or to works completely rewritten in the same form."@en .

<http://rdaregistry.info/Elements/w/P10065> a rdf:Property ;
    rdfs:label "has creator"@en,
        "har skapare"@sv ;
    rdakit:instructionNumber "19.2" ;
    rdakit:toolkitDefinition "An agent responsible for the creation of a work."@en,
        "Una persona, familia o entidad corporativa responsable de la creación de una obra."@es,
        "Personne, famille ou collectivité responsable de la création d’une œuvre."@fr ;
    rdakit:toolkitLabel "creator"@en,
        "creador"@es,
        "créateur"@fr,
        "skapare"@sv ;
    reg:hasSubproperty <http://rdaregistry.info/Elements/w/P10001>,
        <http://rdaregistry.info/Elements/w/P10017>,
        <http://rdaregistry.info/Elements/w/P10045>,
        <http://rdaregistry.info/Elements/w/P10050>,
        <http://rdaregistry.info/Elements/w/P10051>,
        <http://rdaregistry.info/Elements/w/P10052>,
        <http://rdaregistry.info/Elements/w/P10053>,
        <http://rdaregistry.info/Elements/w/P10054>,
        <http://rdaregistry.info/Elements/w/P10055>,
        <http://rdaregistry.info/Elements/w/P10056>,
        <http://rdaregistry.info/Elements/w/P10057>,
        <http://rdaregistry.info/Elements/w/P10058>,
        <http://rdaregistry.info/Elements/w/P10059>,
        <http://rdaregistry.info/Elements/w/P10060>,
        <http://rdaregistry.info/Elements/w/P10061>,
        <http://rdaregistry.info/Elements/w/P10062>,
        <http://rdaregistry.info/Elements/w/P10063>,
        <http://rdaregistry.info/Elements/w/P10306>,
        <http://rdaregistry.info/Elements/w/object/P10065> ;
    reg:hasUnconstrained <http://rdaregistry.info/Elements/u/P60447> ;
    reg:lexicalAlias <http://rdaregistry.info/Elements/w/creator.en> ;
    reg:name "creator"@en ;
    reg:status <http://metadataregistry.org/uri/RegStatus/1001> ;
    rdfs:domain <http://rdaregistry.info/Elements/c/C10001> ;
    rdfs:isDefinedBy <http://rdaregistry.info/Elements/w/> ;
    rdfs:subPropertyOf <http://rdaregistry.info/Elements/w/P10311> ;
    skos:definition "Relates a work to an agent responsible for the creation of a work."@en ;
    skos:scopeNote "Creators include agents who are jointly responsible for the creation of a work either performing the same role, such as in a collaboration between two writers, or performing different roles, such as in a collaboration between a composer and a lyricist."@en .

<http://rdaregistry.info/Elements/w/P10047> a rdf:Property ;
    rdfs:label "has other agent associated with work"@en,
        "har övrig person, familj/släkt eller institution knuten till ett verk"@sv ;
    rdakit:instructionNumber "19.3" ;
    rdakit:toolkitDefinition "An agent other than a creator associated with a work."@en,
        "Una persona, familia o entidad corporativa asociada con una obra en una relación diferente de la del creador."@es,
        "Personne, famille ou collectivité associée à une œuvre autrement que comme créateur."@fr ;
    rdakit:toolkitLabel "other agent associated with work"@en,
        "otra persona, familia o entidad corporativa asociada con una obra"@es,
        "autre personne, famille ou collectivité associée à une œuvre"@fr,
        "övrig person, familj/släkt eller institution knuten till ett verk"@sv ;
    reg:hasSubproperty <http://rdaregistry.info/Elements/w/P10006>,
        <http://rdaregistry.info/Elements/w/P10007>,
        <http://rdaregistry.info/Elements/w/P10008>,
        <http://rdaregistry.info/Elements/w/P10011>,
        <http://rdaregistry.info/Elements/w/P10018>,
        <http://rdaregistry.info/Elements/w/P10036>,
        <http://rdaregistry.info/Elements/w/P10037>,
        <http://rdaregistry.info/Elements/w/P10038>,
        <http://rdaregistry.info/Elements/w/P10039>,
        <http://rdaregistry.info/Elements/w/P10040>,
        <http://rdaregistry.info/Elements/w/P10041>,
        <http://rdaregistry.info/Elements/w/P10044>,
        <http://rdaregistry.info/Elements/w/P10046>,
        <http://rdaregistry.info/Elements/w/P10048>,
        <http://rdaregistry.info/Elements/w/P10049>,
        <http://rdaregistry.info/Elements/w/P10064>,
        <http://rdaregistry.info/Elements/w/P10066>,
        <http://rdaregistry.info/Elements/w/P10067>,
        <http://rdaregistry.info/Elements/w/P10068>,
        <http://rdaregistry.info/Elements/w/P10069>,
        <http://rdaregistry.info/Elements/w/P10070>,
        <http://rdaregistry.info/Elements/w/P10071>,
        <http://rdaregistry.info/Elements/w/P10284>,
        <http://rdaregistry.info/Elements/w/P10287>,
        <http://rdaregistry.info/Elements/w/P10292>,
        <http://rdaregistry.info/Elements/w/P10293>,
        <http://rdaregistry.info/Elements/w/P10297>,
        <http://rdaregistry.info/Elements/w/P10298>,
        <http://rdaregistry.info/Elements/w/P10299>,
        <http://rdaregistry.info/Elements/w/P10305>,
        <http://rdaregistry.info/Elements/w/object/P10047> ;
    reg:hasUnconstrained <http://rdaregistry.info/Elements/u/P60374> ;
    reg:lexicalAlias <http://rdaregistry.info/Elements/w/otherAgentWork.en> ;
    reg:name "otherAgentWork"@en ;
    reg:status <http://metadataregistry.org/uri/RegStatus/1001> ;
    rdfs:domain <http://rdaregistry.info/Elements/c/C10001> ;
    rdfs:isDefinedBy <http://rdaregistry.info/Elements/w/> ;
    rdfs:subPropertyOf <http://rdaregistry.info/Elements/w/P10311> ;
    skos:definition "Relates a work to an agent other than a creator associated with a work."@en ;
    skos:scopeNote "Agents to whom correspondence is addressed, agents honoured by a festschrift, directors, cinematographers, sponsoring bodies, production companies, institutions, etc., hosting an exhibition or event, etc., are included."@en .

<http://metadataregistry.org/uri/RegStatus/1001> a skos:Concept ;
    skos:prefLabel "Published"@en .

<http://rdaregistry.info/Elements/w/> dc:title "RDA Work properties"@en ;
    skos:note "Properties derived from RDA elements and relationship designators with the domain of RDA Work."@en ;
    foaf:homepage <http://www.rdaregistry.info/Elements/w/> .

