@prefix rdf: <http://www.w3.org/1999/02/22-rdf-syntax-ns#> .
@prefix dc: <http://purl.org/dc/elements/1.1/> .
@prefix reg: <http://metadataregistry.org/uri/profile/regap/> .
@prefix skos: <http://www.w3.org/2004/02/skos/core#> .

<http://metadataregistry.org/uri/RegStatus/1008>
    a skos:Concept ;
    skos:prefLabel "Deprecated"@en .

<http://rdaregistry.info/termList/extent>
    dc:title "RDA Extent (Deprecated)" ;
    a skos:ConceptScheme .

<http://rdaregistry.info/termList/extent/1002>
    reg:identifier <http://metadataregistry.org/concepts/3278> ;
    reg:status <http://metadataregistry.org/uri/RegStatus/1008> ;
    a skos:Concept ;
    skos:definition "A cartridge containing an audio tape.  (Deprecated)"@en ;
    skos:inScheme <http://rdaregistry.info/termList/extent> ;
    skos:prefLabel "audio cartridge (Deprecated)"@en .

<http://rdaregistry.info/termList/extent/1003>
    reg:identifier <http://metadataregistry.org/concepts/3279> ;
    reg:status <http://metadataregistry.org/uri/RegStatus/1008> ;
    a skos:Concept ;
    skos:definition "Cartridges containing an audio tape.  (Deprecated)"@en ;
    skos:inScheme <http://rdaregistry.info/termList/extent> ;
    skos:prefLabel "audio cartridges (Deprecated)"@en .

<http://rdaregistry.info/termList/extent/1004>
    reg:identifier <http://metadataregistry.org/concepts/3280> ;
    reg:status <http://metadataregistry.org/uri/RegStatus/1008> ;
    a skos:Concept ;
    skos:definition "A roller-shaped object on which sound waves are incised or indented in a continuous circular groove. (Deprecated)"@en ;
    skos:inScheme <http://rdaregistry.info/termList/extent> ;
    skos:prefLabel "audio cylinder (Deprecated)"@en ;
    skos:scopeNote "Includes wax cylinders, wire cylinders, etc. "@en .

<http://rdaregistry.info/termList/extent/1005>
    reg:identifier <http://metadataregistry.org/concepts/3281> ;
    reg:status <http://metadataregistry.org/uri/RegStatus/1008> ;
    a skos:Concept ;
    skos:definition "Roller-shaped objects on which sound waves are incised or indented in a continuous circular groove. (Deprecated)"@en ;
    skos:inScheme <http://rdaregistry.info/termList/extent> ;
    skos:prefLabel "audio cylinders (Deprecated)"@en ;
    skos:scopeNote "Includes wax cylinders, wire cylinders, etc. "@en .

<http://rdaregistry.info/termList/extent/1006>
    reg:identifier <http://metadataregistry.org/concepts/3282> ;
    reg:status <http://metadataregistry.org/uri/RegStatus/1008> ;
    a skos:Concept ;
    skos:altLabel "sound disc (Deprecated)"@en ;
    skos:definition "A disc on which sound waves, recorded as modulations, pulses, etc., are incised or indented in a continuous spiral groove. (Deprecated)"@en ;
    skos:inScheme <http://rdaregistry.info/termList/extent> ;
    skos:prefLabel "audio disc (Deprecated)"@en .

<http://rdaregistry.info/termList/extent/1007>
    reg:identifier <http://metadataregistry.org/concepts/3283> ;
    reg:status <http://metadataregistry.org/uri/RegStatus/1008> ;
    a skos:Concept ;
    skos:altLabel "sound discs (Deprecated)"@en ;
    skos:definition "Discs on which sound waves, recorded as modulations, pulses, etc., are incised or indented in a continuous spiral groove.  (Deprecated)"@en ;
    skos:inScheme <http://rdaregistry.info/termList/extent> ;
    skos:prefLabel "audio discs (Deprecated)"@en .

<http://rdaregistry.info/termList/extent/1008>
    reg:identifier <http://metadataregistry.org/concepts/3284> ;
    reg:status <http://metadataregistry.org/uri/RegStatus/1008> ;
    a skos:Concept ;
    skos:altLabel "piano roll (Deprecated)"@en ;
    skos:definition "A roll of paper on which musical notes are represented by perforations, designed to mechanically reproduce the music when used in a player piano, player organ, etc (Deprecated)"@en ;
    skos:inScheme <http://rdaregistry.info/termList/extent> ;
    skos:prefLabel "audio roll (Deprecated)"@en ;
    skos:scopeNote "Use for piano rolls, etc. "@en .

<http://rdaregistry.info/termList/extent/1009>
    reg:identifier <http://metadataregistry.org/concepts/3285> ;
    reg:status <http://metadataregistry.org/uri/RegStatus/1008> ;
    a skos:Concept ;
    skos:altLabel "piano rolls (Deprecated)"@en ;
    skos:definition "Rolls of paper on which musical notes are represented by perforations, designed to mechanically reproduce the music when used in a player piano, player organ, etc.  (Deprecated)"@en ;
    skos:inScheme <http://rdaregistry.info/termList/extent> ;
    skos:prefLabel "audio rolls (Deprecated)"@en ;
    skos:scopeNote "Use for piano rolls, etc. "@en .

<http://rdaregistry.info/termList/extent/1010>
    reg:identifier <http://metadataregistry.org/concepts/3286> ;
    reg:status <http://metadataregistry.org/uri/RegStatus/1008> ;
    a skos:Concept ;
    skos:definition "A cassette containing an audio tape. (Deprecated)"@en ;
    skos:inScheme <http://rdaregistry.info/termList/extent> ;
    skos:prefLabel "audiocassette (Deprecated)"@en .

<http://rdaregistry.info/termList/extent/1011>
    reg:identifier <http://metadataregistry.org/concepts/3287> ;
    reg:status <http://metadataregistry.org/uri/RegStatus/1008> ;
    a skos:Concept ;
    skos:definition "Cassettes containing an audio tape.  (Deprecated)"@en ;
    skos:inScheme <http://rdaregistry.info/termList/extent> ;
    skos:prefLabel "audiocassettes (Deprecated)"@en .

<http://rdaregistry.info/termList/extent/1012>
    reg:identifier <http://metadataregistry.org/concepts/3288> ;
    reg:status <http://metadataregistry.org/uri/RegStatus/1008> ;
    a skos:Concept ;
    skos:definition "An open reel holding a length of audio tape to be used with reel-to-reel audio equipment. (Deprecated)"@en ;
    skos:inScheme <http://rdaregistry.info/termList/extent> ;
    skos:prefLabel "audiotape reel (Deprecated)"@en .

<http://rdaregistry.info/termList/extent/1013>
    reg:identifier <http://metadataregistry.org/concepts/3289> ;
    reg:status <http://metadataregistry.org/uri/RegStatus/1008> ;
    a skos:Concept ;
    skos:definition "Open reels holding a length of audio tape to be used with reel-to-reel audio equipment.  (Deprecated)"@en ;
    skos:inScheme <http://rdaregistry.info/termList/extent> ;
    skos:prefLabel "audiotape reels (Deprecated)"@en .

<http://rdaregistry.info/termList/extent/1015>
    reg:identifier <http://metadataregistry.org/concepts/3290> ;
    reg:status <http://metadataregistry.org/uri/RegStatus/1008> ;
    a skos:Concept ;
    skos:definition "An open reel holding a length of film on which sound is recorded. (Deprecated)"@en ;
    skos:inScheme <http://rdaregistry.info/termList/extent> ;
    skos:prefLabel "sound-track reel (Deprecated)"@en ;
    skos:scopeNote "Use for sound-track films, whether or not they are intended to accompany visual images on film."@en .

<http://rdaregistry.info/termList/extent/1016>
    reg:identifier <http://metadataregistry.org/concepts/3291> ;
    reg:status <http://metadataregistry.org/uri/RegStatus/1008> ;
    a skos:Concept ;
    skos:definition "Open reels holding a length of film on which sound is recorded. (Deprecated)"@en ;
    skos:inScheme <http://rdaregistry.info/termList/extent> ;
    skos:prefLabel "sound-track reels (Deprecated)"@en ;
    skos:scopeNote "Use for sound-track films, whether or not they are intended to accompany visual images on film."@en .

<http://rdaregistry.info/termList/extent/1017>
    reg:identifier <http://metadataregistry.org/concepts/3292> ;
    reg:status <http://metadataregistry.org/uri/RegStatus/1008> ;
    a skos:Concept ;
    skos:definition "A card containing digitally encoded data designed for use with a computer. (Deprecated)"@en ;
    skos:inScheme <http://rdaregistry.info/termList/extent> ;
    skos:prefLabel "computer card (Deprecated)"@en .

<http://rdaregistry.info/termList/extent/1018>
    reg:identifier <http://metadataregistry.org/concepts/3293> ;
    reg:status <http://metadataregistry.org/uri/RegStatus/1008> ;
    a skos:Concept ;
    skos:definition "Cards containing digitally encoded data designed for use with a computer. (Deprecated)"@en ;
    skos:inScheme <http://rdaregistry.info/termList/extent> ;
    skos:prefLabel "computer cards (Deprecated)"@en .

<http://rdaregistry.info/termList/extent/1019>
    reg:identifier <http://metadataregistry.org/concepts/3294> ;
    reg:status <http://metadataregistry.org/uri/RegStatus/1008> ;
    a skos:Concept ;
    skos:definition "A cartridge containing a miniaturized electronic circuit on a small wafer of semiconductor silicon. (Deprecated)"@en ;
    skos:inScheme <http://rdaregistry.info/termList/extent> ;
    skos:prefLabel "computer chip cartridge (Deprecated)"@en .

<http://rdaregistry.info/termList/extent/1020>
    reg:identifier <http://metadataregistry.org/concepts/3295> ;
    reg:status <http://metadataregistry.org/uri/RegStatus/1008> ;
    a skos:Concept ;
    skos:definition "Cartridges containing a miniaturized electronic circuit on a small wafer of semiconductor silicon. (Deprecated)"@en ;
    skos:inScheme <http://rdaregistry.info/termList/extent> ;
    skos:prefLabel "computer chip cartridges (Deprecated)"@en .

<http://rdaregistry.info/termList/extent/1021>
    reg:identifier <http://metadataregistry.org/concepts/3296> ;
    reg:status <http://metadataregistry.org/uri/RegStatus/1008> ;
    a skos:Concept ;
    skos:definition "A disc containing digitally encoded data, magnetically or optically recorded. (Deprecated)"@en ;
    skos:inScheme <http://rdaregistry.info/termList/extent> ;
    skos:prefLabel "computer disc (Deprecated)"@en .

<http://rdaregistry.info/termList/extent/1022>
    reg:identifier <http://metadataregistry.org/concepts/3297> ;
    reg:status <http://metadataregistry.org/uri/RegStatus/1008> ;
    a skos:Concept ;
    skos:definition "Discs containing digitally encoded data, magnetically or optically recorded. (Deprecated)"@en ;
    skos:inScheme <http://rdaregistry.info/termList/extent> ;
    skos:prefLabel "computer discs (Deprecated)"@en .

<http://rdaregistry.info/termList/extent/1023>
    reg:identifier <http://metadataregistry.org/concepts/3298> ;
    reg:status <http://metadataregistry.org/uri/RegStatus/1008> ;
    a skos:Concept ;
    skos:definition "A cartridge containing one or more computer discs. (Deprecated)"@en ;
    skos:inScheme <http://rdaregistry.info/termList/extent> ;
    skos:prefLabel "computer disc cartridge (Deprecated)"@en .

<http://rdaregistry.info/termList/extent/1024>
    reg:identifier <http://metadataregistry.org/concepts/3299> ;
    reg:status <http://metadataregistry.org/uri/RegStatus/1008> ;
    a skos:Concept ;
    skos:definition "Cartridges containing one or more computer discs. (Deprecated)"@en ;
    skos:inScheme <http://rdaregistry.info/termList/extent> ;
    skos:prefLabel "computer disc cartridges (Deprecated)"@en .

<http://rdaregistry.info/termList/extent/1025>
    reg:identifier <http://metadataregistry.org/concepts/3300> ;
    reg:status <http://metadataregistry.org/uri/RegStatus/1008> ;
    a skos:Concept ;
    skos:definition "A cartridge containing a computer tape. (Deprecated)"@en ;
    skos:inScheme <http://rdaregistry.info/termList/extent> ;
    skos:prefLabel "computer tape cartridge (Deprecated)"@en .

<http://rdaregistry.info/termList/extent/1026>
    reg:identifier <http://metadataregistry.org/concepts/3301> ;
    reg:status <http://metadataregistry.org/uri/RegStatus/1008> ;
    a skos:Concept ;
    skos:definition "Cartridges containing a computer tape. (Deprecated)"@en ;
    skos:inScheme <http://rdaregistry.info/termList/extent> ;
    skos:prefLabel "computer tape cartridges (Deprecated)"@en .

<http://rdaregistry.info/termList/extent/1027>
    reg:identifier <http://metadataregistry.org/concepts/3302> ;
    reg:status <http://metadataregistry.org/uri/RegStatus/1008> ;
    a skos:Concept ;
    skos:definition "A cassette containing a computer tape. (Deprecated)"@en ;
    skos:inScheme <http://rdaregistry.info/termList/extent> ;
    skos:prefLabel "computer tape cassette (Deprecated)"@en .

<http://rdaregistry.info/termList/extent/1028>
    reg:identifier <http://metadataregistry.org/concepts/3303> ;
    reg:status <http://metadataregistry.org/uri/RegStatus/1008> ;
    a skos:Concept ;
    skos:definition "Cassettes containing a computer tape. (Deprecated)"@en ;
    skos:inScheme <http://rdaregistry.info/termList/extent> ;
    skos:prefLabel "computer tape cassettes (Deprecated)"@en .

<http://rdaregistry.info/termList/extent/1029>
    reg:identifier <http://metadataregistry.org/concepts/3304> ;
    reg:status <http://metadataregistry.org/uri/RegStatus/1008> ;
    a skos:Concept ;
    skos:definition "An open reel holding a length of computer tape to be used with a computer tape drive. (Deprecated)"@en ;
    skos:inScheme <http://rdaregistry.info/termList/extent> ;
    skos:prefLabel "computer tape reel (Deprecated)"@en .

<http://rdaregistry.info/termList/extent/1030>
    reg:identifier <http://metadataregistry.org/concepts/3305> ;
    reg:status <http://metadataregistry.org/uri/RegStatus/1008> ;
    a skos:Concept ;
    skos:definition "Open reels holding a length of computer tape to be used with a computer tape drive. (Deprecated)"@en ;
    skos:inScheme <http://rdaregistry.info/termList/extent> ;
    skos:prefLabel "computer tape reels (Deprecated)"@en .

<http://rdaregistry.info/termList/extent/1031>
    reg:identifier <http://metadataregistry.org/concepts/3306> ;
    reg:status <http://metadataregistry.org/uri/RegStatus/1008> ;
    a skos:Concept ;
    skos:definition "A digital resource accessed by means of hardware and software connections to a communications network. (Deprecated)"@en ;
    skos:inScheme <http://rdaregistry.info/termList/extent> ;
    skos:prefLabel "online resource (Deprecated)"@en .

<http://rdaregistry.info/termList/extent/1032>
    reg:identifier <http://metadataregistry.org/concepts/3307> ;
    reg:status <http://metadataregistry.org/uri/RegStatus/1008> ;
    a skos:Concept ;
    skos:definition "Digital resources accessed by means of hardware and software connections to a communications network. (Deprecated)"@en ;
    skos:inScheme <http://rdaregistry.info/termList/extent> ;
    skos:prefLabel "online resources (Deprecated)"@en .

<http://rdaregistry.info/termList/extent/1033>
    reg:identifier <http://metadataregistry.org/concepts/3308> ;
    reg:status <http://metadataregistry.org/uri/RegStatus/1008> ;
    a skos:Concept ;
    skos:definition "A card with one or more rectangular openings or apertures holding frames of microfilm. (Deprecated)"@en ;
    skos:inScheme <http://rdaregistry.info/termList/extent> ;
    skos:prefLabel "aperture card (Deprecated)"@en .

<http://rdaregistry.info/termList/extent/1034>
    reg:identifier <http://metadataregistry.org/concepts/3309> ;
    reg:status <http://metadataregistry.org/uri/RegStatus/1008> ;
    a skos:Concept ;
    skos:definition "Cards with one or more rectangular openings or apertures holding frames of microfilm. (Deprecated)"@en ;
    skos:inScheme <http://rdaregistry.info/termList/extent> ;
    skos:prefLabel "aperture cards (Deprecated)"@en .

<http://rdaregistry.info/termList/extent/1035>
    reg:identifier <http://metadataregistry.org/concepts/3310> ;
    reg:status <http://metadataregistry.org/uri/RegStatus/1008> ;
    a skos:Concept ;
    skos:definition "A sheet of film bearing a number of microimages in a two-dimensional array. (Deprecated)"@en ;
    skos:inScheme <http://rdaregistry.info/termList/extent> ;
    skos:prefLabel "microfiche (Deprecated)"@en .

<http://rdaregistry.info/termList/extent/1036>
    reg:identifier <http://metadataregistry.org/concepts/3311> ;
    reg:status <http://metadataregistry.org/uri/RegStatus/1008> ;
    a skos:Concept ;
    skos:definition "Sheets of film bearing a number of microimages in a two-dimensional array. (Deprecated)"@en ;
    skos:inScheme <http://rdaregistry.info/termList/extent> ;
    skos:prefLabel "microfiches (Deprecated)"@en .

<http://rdaregistry.info/termList/extent/1037>
    reg:identifier <http://metadataregistry.org/concepts/3312> ;
    reg:status <http://metadataregistry.org/uri/RegStatus/1008> ;
    a skos:Concept ;
    skos:definition "A cassette containing uncut microfiches. (Deprecated)"@en ;
    skos:inScheme <http://rdaregistry.info/termList/extent> ;
    skos:prefLabel "microfiche cassette (Deprecated)"@en .

<http://rdaregistry.info/termList/extent/1038>
    reg:identifier <http://metadataregistry.org/concepts/3313> ;
    reg:status <http://metadataregistry.org/uri/RegStatus/1008> ;
    a skos:Concept ;
    skos:definition "Cassettes containing uncut microfiches. (Deprecated)"@en ;
    skos:inScheme <http://rdaregistry.info/termList/extent> ;
    skos:prefLabel "microfiche cassettes (Deprecated)"@en .

<http://rdaregistry.info/termList/extent/1041>
    reg:identifier <http://metadataregistry.org/concepts/3316> ;
    reg:status <http://metadataregistry.org/uri/RegStatus/1008> ;
    a skos:Concept ;
    skos:definition "A cartridge containing a microfilm. (Deprecated)"@en ;
    skos:inScheme <http://rdaregistry.info/termList/extent> ;
    skos:prefLabel "microfilm cartridge (Deprecated)"@en .

<http://rdaregistry.info/termList/extent/1042>
    reg:identifier <http://metadataregistry.org/concepts/3317> ;
    reg:status <http://metadataregistry.org/uri/RegStatus/1008> ;
    a skos:Concept ;
    skos:definition "Cartridges containing a microfilm. (Deprecated)"@en ;
    skos:inScheme <http://rdaregistry.info/termList/extent> ;
    skos:prefLabel "microfilm cartridges (Deprecated)"@en .

<http://rdaregistry.info/termList/extent/1043>
    reg:identifier <http://metadataregistry.org/concepts/3318> ;
    reg:status <http://metadataregistry.org/uri/RegStatus/1008> ;
    a skos:Concept ;
    skos:definition "A cassette containing a microfilm. (Deprecated)"@en ;
    skos:inScheme <http://rdaregistry.info/termList/extent> ;
    skos:prefLabel "microfilm cassette (Deprecated)"@en .

<http://rdaregistry.info/termList/extent/1044>
    reg:identifier <http://metadataregistry.org/concepts/3319> ;
    reg:status <http://metadataregistry.org/uri/RegStatus/1008> ;
    a skos:Concept ;
    skos:definition "Cassettes containing a microfilm. (Deprecated)"@en ;
    skos:inScheme <http://rdaregistry.info/termList/extent> ;
    skos:prefLabel "microfilm cassettes (Deprecated)"@en .

<http://rdaregistry.info/termList/extent/1045>
    reg:identifier <http://metadataregistry.org/concepts/3320> ;
    reg:status <http://metadataregistry.org/uri/RegStatus/1008> ;
    a skos:Concept ;
    skos:definition "An open reel holding a microfilm, to be threaded into a microfilm reader. (Deprecated)"@en ;
    skos:inScheme <http://rdaregistry.info/termList/extent> ;
    skos:prefLabel "microfilm reel (Deprecated)"@en .

<http://rdaregistry.info/termList/extent/1046>
    reg:identifier <http://metadataregistry.org/concepts/3321> ;
    reg:status <http://metadataregistry.org/uri/RegStatus/1008> ;
    a skos:Concept ;
    skos:definition "Open reels holding a microfilm, to be threaded into a microfilm reader. (Deprecated)"@en ;
    skos:inScheme <http://rdaregistry.info/termList/extent> ;
    skos:prefLabel "microfilm reels (Deprecated)"@en .

<http://rdaregistry.info/termList/extent/1047>
    reg:identifier <http://metadataregistry.org/concepts/3322> ;
    reg:status <http://metadataregistry.org/uri/RegStatus/1008> ;
    a skos:Concept ;
    skos:definition "A wound length of microfilm. (Deprecated)"@en ;
    skos:inScheme <http://rdaregistry.info/termList/extent> ;
    skos:prefLabel "microfilm roll (Deprecated)"@en .

<http://rdaregistry.info/termList/extent/1048>
    reg:identifier <http://metadataregistry.org/concepts/3323> ;
    reg:status <http://metadataregistry.org/uri/RegStatus/1008> ;
    a skos:Concept ;
    skos:definition "Wound lengths of microfilm. (Deprecated)"@en ;
    skos:inScheme <http://rdaregistry.info/termList/extent> ;
    skos:prefLabel "microfilm rolls (Deprecated)"@en .

<http://rdaregistry.info/termList/extent/1049>
    reg:identifier <http://metadataregistry.org/concepts/3324> ;
    reg:status <http://metadataregistry.org/uri/RegStatus/1008> ;
    a skos:Concept ;
    skos:definition "A short strip of microfilm cut from a roll. (Deprecated)"@en ;
    skos:inScheme <http://rdaregistry.info/termList/extent> ;
    skos:prefLabel "microfilm slip (Deprecated)"@en .

<http://rdaregistry.info/termList/extent/1050>
    reg:identifier <http://metadataregistry.org/concepts/3325> ;
    reg:status <http://metadataregistry.org/uri/RegStatus/1008> ;
    a skos:Concept ;
    skos:definition "Short strips of microfilm cut from a roll. (Deprecated)"@en ;
    skos:inScheme <http://rdaregistry.info/termList/extent> ;
    skos:prefLabel "microfilm slips (Deprecated)"@en .

<http://rdaregistry.info/termList/extent/1051>
    reg:identifier <http://metadataregistry.org/concepts/3326> ;
    reg:status <http://metadataregistry.org/uri/RegStatus/1008> ;
    a skos:Concept ;
    skos:definition "A card or sheet of opaque material bearing a number of microimages in a two-dimensional array. (Deprecated)"@en ;
    skos:inScheme <http://rdaregistry.info/termList/extent> ;
    skos:prefLabel "microopaque (Deprecated)"@en .

<http://rdaregistry.info/termList/extent/1052>
    reg:identifier <http://metadataregistry.org/concepts/3327> ;
    reg:status <http://metadataregistry.org/uri/RegStatus/1008> ;
    a skos:Concept ;
    skos:definition "Cards or sheets of opaque material bearing a number of microimages in a two-dimensional array. (Deprecated)"@en ;
    skos:inScheme <http://rdaregistry.info/termList/extent> ;
    skos:prefLabel "microopaques (Deprecated)"@en .

<http://rdaregistry.info/termList/extent/1053>
    reg:identifier <http://metadataregistry.org/concepts/3328> ;
    reg:status <http://metadataregistry.org/uri/RegStatus/1008> ;
    a skos:Concept ;
    skos:definition "A small sheet of transparent material (with or without a protective mount) bearing a minute object designed for use with a device such as a microscope.  (Deprecated)"@en ;
    skos:inScheme <http://rdaregistry.info/termList/extent> ;
    skos:prefLabel "microscope slide (Deprecated)"@en ;
    skos:related <http://rdaregistry.info/termList/extent/1071> .

<http://rdaregistry.info/termList/extent/1054>
    reg:identifier <http://metadataregistry.org/concepts/3329> ;
    reg:status <http://metadataregistry.org/uri/RegStatus/1008> ;
    a skos:Concept ;
    skos:definition "Small sheets of transparent material (with or without a protective mount) bearing a minute object designed for use with a device such as a microscope.  (Deprecated)"@en ;
    skos:inScheme <http://rdaregistry.info/termList/extent> ;
    skos:prefLabel "microscope slides (Deprecated)"@en ;
    skos:related <http://rdaregistry.info/termList/extent/1072> .

<http://rdaregistry.info/termList/extent/1055>
    reg:identifier <http://metadataregistry.org/concepts/3330> ;
    reg:status <http://metadataregistry.org/uri/RegStatus/1008> ;
    a skos:Concept ;
    skos:definition "A cartridge containing a motion picture film. (Deprecated)"@en ;
    skos:inScheme <http://rdaregistry.info/termList/extent> ;
    skos:prefLabel "film cartridge (Deprecated)"@en .

<http://rdaregistry.info/termList/extent/1056>
    reg:identifier <http://metadataregistry.org/concepts/3331> ;
    reg:status <http://metadataregistry.org/uri/RegStatus/1008> ;
    a skos:Concept ;
    skos:definition "Cartridges containing a motion picture film. (Deprecated)"@en ;
    skos:inScheme <http://rdaregistry.info/termList/extent> ;
    skos:prefLabel "film cartridges (Deprecated)"@en .

<http://rdaregistry.info/termList/extent/1057>
    reg:identifier <http://metadataregistry.org/concepts/3332> ;
    reg:status <http://metadataregistry.org/uri/RegStatus/1008> ;
    a skos:Concept ;
    skos:definition "A cassette containing a motion picture film. (Deprecated)"@en ;
    skos:inScheme <http://rdaregistry.info/termList/extent> ;
    skos:prefLabel "film cassette (Deprecated)"@en .

<http://rdaregistry.info/termList/extent/1058>
    reg:identifier <http://metadataregistry.org/concepts/3333> ;
    reg:status <http://metadataregistry.org/uri/RegStatus/1008> ;
    a skos:Concept ;
    skos:definition "Cassettes containing a motion picture film. (Deprecated)"@en ;
    skos:inScheme <http://rdaregistry.info/termList/extent> ;
    skos:prefLabel "film cassettes (Deprecated)"@en .

<http://rdaregistry.info/termList/extent/1059>
    reg:identifier <http://metadataregistry.org/concepts/3334> ;
    reg:status <http://metadataregistry.org/uri/RegStatus/1008> ;
    a skos:Concept ;
    skos:definition "An open reel holding a motion picture film to be used with a motion picture film projector. (Deprecated)"@en ;
    skos:inScheme <http://rdaregistry.info/termList/extent> ;
    skos:prefLabel "film reel (Deprecated)"@en .

<http://rdaregistry.info/termList/extent/1060>
    reg:identifier <http://metadataregistry.org/concepts/3335> ;
    reg:status <http://metadataregistry.org/uri/RegStatus/1008> ;
    a skos:Concept ;
    skos:definition "Open reels holding a motion picture film to be used with a motion picture film projector. (Deprecated)"@en ;
    skos:inScheme <http://rdaregistry.info/termList/extent> ;
    skos:prefLabel "film reels (Deprecated)"@en .

<http://rdaregistry.info/termList/extent/1061>
    reg:identifier <http://metadataregistry.org/concepts/3336> ;
    reg:status <http://metadataregistry.org/uri/RegStatus/1008> ;
    a skos:Concept ;
    skos:definition "A wound length of film. (Deprecated)"@en ;
    skos:inScheme <http://rdaregistry.info/termList/extent> ;
    skos:prefLabel "film roll (Deprecated)"@en .

<http://rdaregistry.info/termList/extent/1062>
    reg:identifier <http://metadataregistry.org/concepts/3337> ;
    reg:status <http://metadataregistry.org/uri/RegStatus/1008> ;
    a skos:Concept ;
    skos:definition "Wound lengths of film. (Deprecated)"@en ;
    skos:inScheme <http://rdaregistry.info/termList/extent> ;
    skos:prefLabel "film rolls (Deprecated)"@en .

<http://rdaregistry.info/termList/extent/1063>
    reg:identifier <http://metadataregistry.org/concepts/3338> ;
    reg:status <http://metadataregistry.org/uri/RegStatus/1008> ;
    a skos:Concept ;
    skos:definition "A short strip of film, usually in rigid format rather than rolled. (Deprecated)"@en ;
    skos:inScheme <http://rdaregistry.info/termList/extent> ;
    skos:prefLabel "filmslip (Deprecated)"@en .

<http://rdaregistry.info/termList/extent/1064>
    reg:identifier <http://metadataregistry.org/concepts/3339> ;
    reg:status <http://metadataregistry.org/uri/RegStatus/1008> ;
    a skos:Concept ;
    skos:definition "Short strips of film, usually in rigid format rather than rolled. (Deprecated)"@en ;
    skos:inScheme <http://rdaregistry.info/termList/extent> ;
    skos:prefLabel "filmslips (Deprecated)"@en .

<http://rdaregistry.info/termList/extent/1065>
    reg:identifier <http://metadataregistry.org/concepts/3340> ;
    reg:status <http://metadataregistry.org/uri/RegStatus/1008> ;
    a skos:Concept ;
    skos:definition "A roll of film, with or without recorded sound, containing a succession of images intended for projection one at a time. (Deprecated)"@en ;
    skos:inScheme <http://rdaregistry.info/termList/extent> ;
    skos:prefLabel "filmstrip (Deprecated)"@en .

<http://rdaregistry.info/termList/extent/1066>
    reg:identifier <http://metadataregistry.org/concepts/3341> ;
    reg:status <http://metadataregistry.org/uri/RegStatus/1008> ;
    a skos:Concept ;
    skos:definition "Rolls of film, with or without recorded sound, containing a succession of images intended for projection one at a time. (Deprecated)"@en ;
    skos:inScheme <http://rdaregistry.info/termList/extent> ;
    skos:prefLabel "filmstrips (Deprecated)"@en .

<http://rdaregistry.info/termList/extent/1067>
    reg:identifier <http://metadataregistry.org/concepts/3342> ;
    reg:status <http://metadataregistry.org/uri/RegStatus/1008> ;
    a skos:Concept ;
    skos:definition "A cartridge containing a filmstrip. (Deprecated)"@en ;
    skos:inScheme <http://rdaregistry.info/termList/extent> ;
    skos:prefLabel "filmstrip cartridge (Deprecated)"@en .

<http://rdaregistry.info/termList/extent/1068>
    reg:identifier <http://metadataregistry.org/concepts/3343> ;
    reg:status <http://metadataregistry.org/uri/RegStatus/1008> ;
    a skos:Concept ;
    skos:definition "Cartridges containing a filmstrip. (Deprecated)"@en ;
    skos:inScheme <http://rdaregistry.info/termList/extent> ;
    skos:prefLabel "filmstrip cartridges (Deprecated)"@en .

<http://rdaregistry.info/termList/extent/1069>
    reg:identifier <http://metadataregistry.org/concepts/3344> ;
    reg:status <http://metadataregistry.org/uri/RegStatus/1008> ;
    a skos:Concept ;
    skos:altLabel "overhead projectural (Deprecated)"@en, "transparency"@en ;
    skos:definition "A sheet of transparent material (with or without a protective mount) bearing an image designed for use with an overhead projector. (Deprecated)"@en ;
    skos:inScheme <http://rdaregistry.info/termList/extent> ;
    skos:prefLabel "overhead transparency (Deprecated)"@en .

<http://rdaregistry.info/termList/extent/1070>
    reg:identifier <http://metadataregistry.org/concepts/3345> ;
    reg:status <http://metadataregistry.org/uri/RegStatus/1008> ;
    a skos:Concept ;
    skos:altLabel "overhead projectural (Deprecated)"@en, "transparencies"@en ;
    skos:definition "Sheets of transparent material (with or without a protective mount) bearing an image designed for use with an overhead projector. (Deprecated)"@en ;
    skos:inScheme <http://rdaregistry.info/termList/extent> ;
    skos:prefLabel "overhead transparencies (Deprecated)"@en .

<http://rdaregistry.info/termList/extent/1071>
    reg:identifier <http://metadataregistry.org/concepts/3346> ;
    reg:status <http://metadataregistry.org/uri/RegStatus/1008> ;
    a skos:Concept ;
    skos:definition "A small sheet of transparent material (usually in a protective mount) bearing an image designed for use with an slide projector or viewer. (Deprecated)"@en ;
    skos:inScheme <http://rdaregistry.info/termList/extent> ;
    skos:prefLabel "slide (Deprecated)"@en ;
    skos:related <http://rdaregistry.info/termList/extent/1053> ;
    skos:scopeNote "For slides designed to be used with a microscope, use microscope slide."@en .

<http://rdaregistry.info/termList/extent/1072>
    reg:identifier <http://metadataregistry.org/concepts/3347> ;
    reg:status <http://metadataregistry.org/uri/RegStatus/1008> ;
    a skos:Concept ;
    skos:definition "Small sheets of transparent material (usually in a protective mount) bearing an image designed for use with an slide projector or viewer. (Deprecated)"@en ;
    skos:inScheme <http://rdaregistry.info/termList/extent> ;
    skos:prefLabel "slides (Deprecated)"@en ;
    skos:related <http://rdaregistry.info/termList/extent/1054> ;
    skos:scopeNote "For slides designed to be used with a microscope, use microscope slides."@en .

<http://rdaregistry.info/termList/extent/1073>
    reg:identifier <http://metadataregistry.org/concepts/3348> ;
    reg:status <http://metadataregistry.org/uri/RegStatus/1008> ;
    a skos:Concept ;
    skos:definition "A card bearing stereographic images. (Deprecated)"@en ;
    skos:inScheme <http://rdaregistry.info/termList/extent> ;
    skos:prefLabel "stereograph card (Deprecated)"@en .

<http://rdaregistry.info/termList/extent/1074>
    reg:identifier <http://metadataregistry.org/concepts/3349> ;
    reg:status <http://metadataregistry.org/uri/RegStatus/1008> ;
    a skos:Concept ;
    skos:definition "Cards bearing stereographic images. (Deprecated)"@en ;
    skos:inScheme <http://rdaregistry.info/termList/extent> ;
    skos:prefLabel "stereograph cards (Deprecated)"@en .

<http://rdaregistry.info/termList/extent/1075>
    reg:identifier <http://metadataregistry.org/concepts/3350> ;
    reg:status <http://metadataregistry.org/uri/RegStatus/1008> ;
    a skos:Concept ;
    skos:definition "A disc with openings around the perimeter holding pairs of still images designed for use with a stereograph viewer. (Deprecated)"@en ;
    skos:inScheme <http://rdaregistry.info/termList/extent> ;
    skos:prefLabel "stereograph disc (Deprecated)"@en .

<http://rdaregistry.info/termList/extent/1076>
    reg:identifier <http://metadataregistry.org/concepts/3351> ;
    reg:status <http://metadataregistry.org/uri/RegStatus/1008> ;
    a skos:Concept ;
    skos:definition "Discs with openings around the perimeter holding pairs of still images designed for use with a stereograph viewer. (Deprecated)"@en ;
    skos:inScheme <http://rdaregistry.info/termList/extent> ;
    skos:prefLabel "stereograph discs (Deprecated)"@en .

<http://rdaregistry.info/termList/extent/1077>
    reg:identifier <http://metadataregistry.org/concepts/3352> ;
    reg:status <http://metadataregistry.org/uri/RegStatus/1008> ;
    a skos:Concept ;
    skos:definition "A small sheet of opaque material. (Deprecated)"@en ;
    skos:inScheme <http://rdaregistry.info/termList/extent> ;
    skos:prefLabel "card (Deprecated)"@en .

<http://rdaregistry.info/termList/extent/1078>
    reg:identifier <http://metadataregistry.org/concepts/3353> ;
    reg:status <http://metadataregistry.org/uri/RegStatus/1008> ;
    a skos:Concept ;
    skos:definition "Small sheets of opaque material. (Deprecated)"@en ;
    skos:inScheme <http://rdaregistry.info/termList/extent> ;
    skos:prefLabel "cards (Deprecated)"@en .

<http://rdaregistry.info/termList/extent/1079>
    reg:identifier <http://metadataregistry.org/concepts/3354> ;
    reg:status <http://metadataregistry.org/uri/RegStatus/1008> ;
    a skos:Concept ;
    skos:definition "A hinging device holding two or more sheets designed for use on an easel. (Deprecated)"@en ;
    skos:inScheme <http://rdaregistry.info/termList/extent> ;
    skos:prefLabel "flipchart (Deprecated)"@en .

<http://rdaregistry.info/termList/extent/1080>
    reg:identifier <http://metadataregistry.org/concepts/3355> ;
    reg:status <http://metadataregistry.org/uri/RegStatus/1008> ;
    a skos:Concept ;
    skos:definition "Hinging devices holding two or more sheets designed for use on an easel. (Deprecated)"@en ;
    skos:inScheme <http://rdaregistry.info/termList/extent> ;
    skos:prefLabel "flipcharts (Deprecated)"@en .

<http://rdaregistry.info/termList/extent/1081>
    reg:identifier <http://metadataregistry.org/concepts/3356> ;
    reg:status <http://metadataregistry.org/uri/RegStatus/1008> ;
    a skos:Concept ;
    skos:definition "A three-dimensional artifact (or a replica of an artifact) or a naturally-occurring object. (Deprecated)"@en ;
    skos:inScheme <http://rdaregistry.info/termList/extent> ;
    skos:prefLabel "object (Deprecated)"@en .

<http://rdaregistry.info/termList/extent/1082>
    reg:identifier <http://metadataregistry.org/concepts/3357> ;
    reg:status <http://metadataregistry.org/uri/RegStatus/1008> ;
    a skos:Concept ;
    skos:definition "Three-dimensional artifacts (or replicas of artifacts) or naturally-occurring objects. (Deprecated)"@en ;
    skos:inScheme <http://rdaregistry.info/termList/extent> ;
    skos:prefLabel "objects (Deprecated)"@en .

<http://rdaregistry.info/termList/extent/1083>
    reg:identifier <http://metadataregistry.org/concepts/3358> ;
    reg:status <http://metadataregistry.org/uri/RegStatus/1008> ;
    a skos:Concept ;
    skos:definition "A wound length of material (paper, film, tape, etc.). (Deprecated)"@en ;
    skos:inScheme <http://rdaregistry.info/termList/extent> ;
    skos:prefLabel "roll (Deprecated)"@en .

<http://rdaregistry.info/termList/extent/1084>
    reg:identifier <http://metadataregistry.org/concepts/3359> ;
    reg:status <http://metadataregistry.org/uri/RegStatus/1008> ;
    a skos:Concept ;
    skos:definition "Wound lengths of material (paper, film, tape, etc.). (Deprecated)"@en ;
    skos:inScheme <http://rdaregistry.info/termList/extent> ;
    skos:prefLabel "rolls (Deprecated)"@en .

<http://rdaregistry.info/termList/extent/1085>
    reg:identifier <http://metadataregistry.org/concepts/3360> ;
    reg:status <http://metadataregistry.org/uri/RegStatus/1008> ;
    a skos:Concept ;
    skos:definition "A flat piece of thin material (paper, plastic, etc.). (Deprecated)"@en ;
    skos:inScheme <http://rdaregistry.info/termList/extent> ;
    skos:prefLabel "sheet (Deprecated)"@en .

<http://rdaregistry.info/termList/extent/1086>
    reg:identifier <http://metadataregistry.org/concepts/3361> ;
    reg:status <http://metadataregistry.org/uri/RegStatus/1008> ;
    a skos:Concept ;
    skos:definition "Flat pieces of thin material (paper, plastic, etc.). (Deprecated)"@en ;
    skos:inScheme <http://rdaregistry.info/termList/extent> ;
    skos:prefLabel "sheets (Deprecated)"@en .

<http://rdaregistry.info/termList/extent/1087>
    reg:identifier <http://metadataregistry.org/concepts/3362> ;
    reg:status <http://metadataregistry.org/uri/RegStatus/1008> ;
    a skos:Concept ;
    skos:definition "One or more sheets bound or fastened together to form a single unit. (Deprecated)"@en ;
    skos:inScheme <http://rdaregistry.info/termList/extent> ;
    skos:prefLabel "volume (Deprecated)"@en .

<http://rdaregistry.info/termList/extent/1088>
    reg:identifier <http://metadataregistry.org/concepts/3363> ;
    reg:status <http://metadataregistry.org/uri/RegStatus/1008> ;
    a skos:Concept ;
    skos:definition "One or more sheets bound or fastened together to form a single units. (Deprecated)"@en ;
    skos:inScheme <http://rdaregistry.info/termList/extent> ;
    skos:prefLabel "volumes (Deprecated)"@en .

<http://rdaregistry.info/termList/extent/1089>
    reg:identifier <http://metadataregistry.org/concepts/3364> ;
    reg:status <http://metadataregistry.org/uri/RegStatus/1008> ;
    a skos:Concept ;
    skos:definition "A cartridge containing a video tape. (Deprecated)"@en ;
    skos:inScheme <http://rdaregistry.info/termList/extent> ;
    skos:prefLabel "video cartridge (Deprecated)"@en .

<http://rdaregistry.info/termList/extent/1090>
    reg:identifier <http://metadataregistry.org/concepts/3365> ;
    reg:status <http://metadataregistry.org/uri/RegStatus/1008> ;
    a skos:Concept ;
    skos:definition "Cartridges containing a video tape. (Deprecated)"@en ;
    skos:inScheme <http://rdaregistry.info/termList/extent> ;
    skos:prefLabel "video cartridges (Deprecated)"@en .

<http://rdaregistry.info/termList/extent/1091>
    reg:identifier <http://metadataregistry.org/concepts/3366> ;
    reg:status <http://metadataregistry.org/uri/RegStatus/1008> ;
    a skos:Concept ;
    skos:definition "Cassettes containing a video tape. (Deprecated)"@en ;
    skos:inScheme <http://rdaregistry.info/termList/extent> ;
    skos:prefLabel "videocassettes (Deprecated)"@en .

<http://rdaregistry.info/termList/extent/1092>
    reg:identifier <http://metadataregistry.org/concepts/3367> ;
    reg:status <http://metadataregistry.org/uri/RegStatus/1008> ;
    a skos:Concept ;
    skos:definition "A cassette containing a video tape. (Deprecated)"@en ;
    skos:inScheme <http://rdaregistry.info/termList/extent> ;
    skos:prefLabel "videocassette (Deprecated)"@en .

<http://rdaregistry.info/termList/extent/1093>
    reg:identifier <http://metadataregistry.org/concepts/3368> ;
    reg:status <http://metadataregistry.org/uri/RegStatus/1008> ;
    a skos:Concept ;
    skos:definition "A disc on which video signals, with or without sound, are recorded. (Deprecated)"@en ;
    skos:inScheme <http://rdaregistry.info/termList/extent> ;
    skos:prefLabel "videodisc (Deprecated)"@en .

<http://rdaregistry.info/termList/extent/1094>
    reg:identifier <http://metadataregistry.org/concepts/3369> ;
    reg:status <http://metadataregistry.org/uri/RegStatus/1008> ;
    a skos:Concept ;
    skos:definition "Discs on which video signals, with or without sound, are recorded. (Deprecated)"@en ;
    skos:inScheme <http://rdaregistry.info/termList/extent> ;
    skos:prefLabel "videodiscs (Deprecated)"@en .

<http://rdaregistry.info/termList/extent/1095>
    reg:identifier <http://metadataregistry.org/concepts/3370> ;
    reg:status <http://metadataregistry.org/uri/RegStatus/1008> ;
    a skos:Concept ;
    skos:definition "An open reel holding a video tape for use with reel-to-reel video equipment. (Deprecated)"@en ;
    skos:inScheme <http://rdaregistry.info/termList/extent> ;
    skos:prefLabel "videotape reel (Deprecated)"@en .

<http://rdaregistry.info/termList/extent/1096>
    reg:identifier <http://metadataregistry.org/concepts/3371> ;
    reg:status <http://metadataregistry.org/uri/RegStatus/1008> ;
    a skos:Concept ;
    skos:definition "Open reels holding a video tape for use with reel-to-reel video equipment. (Deprecated)"@en ;
    skos:inScheme <http://rdaregistry.info/termList/extent> ;
    skos:prefLabel "videotape reels (Deprecated)"@en .

