@prefix rdf: <http://www.w3.org/1999/02/22-rdf-syntax-ns#> .
@prefix dc: <http://purl.org/dc/elements/1.1/> .
@prefix reg: <http://metadataregistry.org/uri/profile/regap/> .
@prefix skos: <http://www.w3.org/2004/02/skos/core#> .

<http://metadataregistry.org/uri/RegStatus/1008>
    a skos:Concept ;
    skos:prefLabel "Deprecated"@en .

<http://rdaregistry.info/termList/extentCarto>
    dc:title "RDA Extent of Cartographic Resource (Deprecated)" ;
    a skos:ConceptScheme .

<http://rdaregistry.info/termList/extentCarto/1001>
    reg:identifier <http://metadataregistry.org/concepts/761> ;
    reg:status <http://metadataregistry.org/uri/RegStatus/1008> ;
    a skos:Concept ;
    skos:definition "A unit of extent of cartographic resource that is a volume of maps or other cartographic content, with or without descriptive text. (Deprecated)"@en ;
    skos:inScheme <http://rdaregistry.info/termList/extentCarto> ;
    skos:prefLabel "atlas (Deprecated)"@en .

<http://rdaregistry.info/termList/extentCarto/1002>
    reg:identifier <http://metadataregistry.org/concepts/762> ;
    reg:status <http://metadataregistry.org/uri/RegStatus/1008> ;
    a skos:Concept ;
    skos:definition "A unit of extent of cartographic resource that is a geographic representation of numeric data, or of the course or results of an action or process. The term is sometimes also applied to maps characterized by much simplified, or schematic, representation. (Deprecated)"@en ;
    skos:inScheme <http://rdaregistry.info/termList/extentCarto> ;
    skos:prefLabel "diagram (Deprecated)"@en .

<http://rdaregistry.info/termList/extentCarto/1003>
    reg:identifier <http://metadataregistry.org/concepts/763> ;
    reg:status <http://metadataregistry.org/uri/RegStatus/1008> ;
    a skos:Concept ;
    skos:definition "A unit of extent of cartographic resource that is a depiction of the Earth or other celestial body (real or imaginary) on the surface of a sphere. (Deprecated)"@en ;
    skos:inScheme <http://rdaregistry.info/termList/extentCarto> ;
    skos:prefLabel "globe (Deprecated)"@en .

<http://rdaregistry.info/termList/extentCarto/1004>
    reg:identifier <http://metadataregistry.org/concepts/764> ;
    reg:status <http://metadataregistry.org/uri/RegStatus/1008> ;
    a skos:Concept ;
    skos:altLabel "plan (cartography) (Deprecated)"@en ;
    skos:definition "A unit of extent of cartographic resource that is a representation, normally to scale and on a two-dimensional medium, of a selection of material or abstract features on, or in relation to, the surface of Earth, another celestial body, or an imaginary place. (Deprecated)"@en ;
    skos:inScheme <http://rdaregistry.info/termList/extentCarto> ;
    skos:prefLabel "map (Deprecated)"@en .

<http://rdaregistry.info/termList/extentCarto/1005>
    reg:identifier <http://metadataregistry.org/concepts/765> ;
    reg:status <http://metadataregistry.org/uri/RegStatus/1008> ;
    a skos:Concept ;
    skos:definition "A unit of extent of cartographic resource that is a three-dimensional representation of the whole or part of the Earth or any celestial body (real or imaginary) at any scale. (Deprecated)"@en ;
    skos:inScheme <http://rdaregistry.info/termList/extentCarto> ;
    skos:prefLabel "model (Deprecated)"@en .

<http://rdaregistry.info/termList/extentCarto/1006>
    reg:identifier <http://metadataregistry.org/concepts/766> ;
    reg:status <http://metadataregistry.org/uri/RegStatus/1008> ;
    a skos:Concept ;
    skos:definition "In cartography, a scale representation of the intersection of a vertical surface (which may or may not be a plane) with the surface of the ground, or of the intersection of such a vertical surface with that of a conceptual three-dimensional model representing phenomena having a continuous distribution (e.g., rainfall). (Deprecated)"@en ;
    skos:inScheme <http://rdaregistry.info/termList/extentCarto> ;
    skos:prefLabel "profile (Deprecated)"@en .

<http://rdaregistry.info/termList/extentCarto/1007>
    reg:identifier <http://metadataregistry.org/concepts/767> ;
    reg:status <http://metadataregistry.org/uri/RegStatus/1008> ;
    a skos:Concept ;
    skos:definition "A unit of extent of cartographic resource that is a pictorial product of any remote-sensing instrument that detects and measures reflected and/or emitted electromagnetic radiation from a distance and reflected underwater sound waves in the case of sonar. (Deprecated)"@en ;
    skos:inScheme <http://rdaregistry.info/termList/extentCarto> ;
    skos:prefLabel "remote-sensing image (Deprecated)"@en .

<http://rdaregistry.info/termList/extentCarto/1008>
    reg:identifier <http://metadataregistry.org/concepts/768> ;
    reg:status <http://metadataregistry.org/uri/RegStatus/1008> ;
    a skos:Concept ;
    skos:altLabel "map section (Deprecated)"@en ;
    skos:definition "A unit of extent of cartographic resource that is a scale representation of a vertical surface (commonly a plane) displaying both the profile where it intersects the surface of a celestial body, or some conceptual model, and the underlying structures along the plane of intersection (e.g., a geological section). (Deprecated)"@en ;
    skos:inScheme <http://rdaregistry.info/termList/extentCarto> ;
    skos:prefLabel "section (Deprecated)"@en .

<http://rdaregistry.info/termList/extentCarto/1009>
    reg:identifier <http://metadataregistry.org/concepts/769> ;
    reg:status <http://metadataregistry.org/uri/RegStatus/1008> ;
    a skos:Concept ;
    skos:definition "A unit of extent of cartographic resource that is a perspective representation of the landscape in which detail is shown as if projected on an oblique plane (e.g., a bird’s-eye view, panorama, panoramic drawing, worm’s-eye view). (Deprecated)"@en ;
    skos:inScheme <http://rdaregistry.info/termList/extentCarto> ;
    skos:prefLabel "view (Deprecated)"@en .

<http://rdaregistry.info/termList/extentCarto/1010>
    reg:identifier <http://metadataregistry.org/concepts/1084> ;
    reg:status <http://metadataregistry.org/uri/RegStatus/1008> ;
    a skos:Concept ;
    skos:definition "Volumes of maps or other cartographic content, with or without descriptive text. (Deprecated)"@en ;
    skos:inScheme <http://rdaregistry.info/termList/extentCarto> ;
    skos:prefLabel "atlases (Deprecated)"@en .

<http://rdaregistry.info/termList/extentCarto/1011>
    reg:identifier <http://metadataregistry.org/concepts/1085> ;
    reg:status <http://metadataregistry.org/uri/RegStatus/1008> ;
    a skos:Concept ;
    skos:inScheme <http://rdaregistry.info/termList/extentCarto> ;
    skos:prefLabel "diagrams (Deprecated)"@en .

<http://rdaregistry.info/termList/extentCarto/1012>
    reg:identifier <http://metadataregistry.org/concepts/1086> ;
    reg:status <http://metadataregistry.org/uri/RegStatus/1008> ;
    a skos:Concept ;
    skos:definition "Depictions of the Earth or other celestial body (real or imaginary) on the surface of a sphere. (Deprecated)"@en ;
    skos:inScheme <http://rdaregistry.info/termList/extentCarto> ;
    skos:prefLabel "globes (Deprecated)"@en .

<http://rdaregistry.info/termList/extentCarto/1013>
    reg:identifier <http://metadataregistry.org/concepts/1087> ;
    reg:status <http://metadataregistry.org/uri/RegStatus/1008> ;
    a skos:Concept ;
    skos:altLabel "plans (cartography) (Deprecated)"@en ;
    skos:definition "Representations, normally to scale and on a two-dimensional medium, of a selection of material or abstract features on, or in relation to, the surface of Earth, another celestial body, or an imaginary place (Deprecated)"@en ;
    skos:inScheme <http://rdaregistry.info/termList/extentCarto> ;
    skos:prefLabel "maps (Deprecated)"@en .

<http://rdaregistry.info/termList/extentCarto/1014>
    reg:identifier <http://metadataregistry.org/concepts/1088> ;
    reg:status <http://metadataregistry.org/uri/RegStatus/1008> ;
    a skos:Concept ;
    skos:definition "Three-dimensional representations of the whole or part of the Earth or any celestial body (real or imaginary) at any scale. (Deprecated)"@en ;
    skos:inScheme <http://rdaregistry.info/termList/extentCarto> ;
    skos:prefLabel "models (Deprecated)"@en .

<http://rdaregistry.info/termList/extentCarto/1015>
    reg:identifier <http://metadataregistry.org/concepts/1089> ;
    reg:status <http://metadataregistry.org/uri/RegStatus/1008> ;
    a skos:Concept ;
    skos:definition "In cartography, scale representations of the intersection of a vertical surface (which may or may not be a plane) with the surface of the ground, or of the intersection of such a vertical surface with that of a conceptual three-dimensional model representing phenomena having a continuous distribution (e.g., rainfall). (Deprecated)"@en ;
    skos:inScheme <http://rdaregistry.info/termList/extentCarto> ;
    skos:prefLabel "profiles (Deprecated)"@en .

<http://rdaregistry.info/termList/extentCarto/1016>
    reg:identifier <http://metadataregistry.org/concepts/1090> ;
    reg:status <http://metadataregistry.org/uri/RegStatus/1008> ;
    a skos:Concept ;
    skos:inScheme <http://rdaregistry.info/termList/extentCarto> ;
    skos:prefLabel "remote sensing images (Deprecated)"@en .

<http://rdaregistry.info/termList/extentCarto/1017>
    reg:identifier <http://metadataregistry.org/concepts/1091> ;
    reg:status <http://metadataregistry.org/uri/RegStatus/1008> ;
    a skos:Concept ;
    skos:altLabel "map sections (Deprecated)"@en ;
    skos:definition "Scale representations of a vertical surface (commonly a plane) displaying both the profile where it intersects the surface of a celestial body, or some conceptual model, and the underlying structures along the plane of intersection (e.g., a geological section). (Deprecated)"@en ;
    skos:inScheme <http://rdaregistry.info/termList/extentCarto> ;
    skos:prefLabel "sections (Deprecated)"@en .

<http://rdaregistry.info/termList/extentCarto/1018>
    reg:identifier <http://metadataregistry.org/concepts/1092> ;
    reg:status <http://metadataregistry.org/uri/RegStatus/1008> ;
    a skos:Concept ;
    skos:definition "In cartography, perspective representations of the landscape in which detail is shown as if projected on an oblique plane (e.g., a bird’s-eye view, panorama, panoramic drawing, worm’s-eye view). (Deprecated)"@en ;
    skos:inScheme <http://rdaregistry.info/termList/extentCarto> ;
    skos:prefLabel "views (Deprecated)"@en .

