@prefix rdf: <http://www.w3.org/1999/02/22-rdf-syntax-ns#> .
@prefix dc: <http://purl.org/dc/elements/1.1/> .
@prefix rdakit: <http://metadataregistry.org/uri/profile/rdakit/> .
@prefix reg: <http://metadataregistry.org/uri/profile/regap/> .
@prefix skos: <http://www.w3.org/2004/02/skos/core#> .

<http://metadataregistry.org/uri/RegStatus/1001>
    a skos:Concept ;
    skos:prefLabel "Published"@en .

<http://rdaregistry.info/termList/presFormat>
    dc:title "RDA Presentation Format" ;
    a skos:ConceptScheme .

<http://rdaregistry.info/termList/presFormat/1001>
    rdakit:toolkitDefinition "A presentation format of a motion picture film that presents an aspect ratio of up to 2.76:1, originally using three synchronized projectors."@en ;
    rdakit:toolkitLabel "Cinerama"@en ;
    reg:identifier <http://metadataregistry.org/concepts/887> ;
    reg:status <http://metadataregistry.org/uri/RegStatus/1001> ;
    a skos:Concept ;
    skos:definition "A presentation format of a motion picture film that presents an aspect ratio of up to 2.76:1, originally using three synchronized projectors."@en ;
    skos:inScheme <http://rdaregistry.info/termList/presFormat> ;
    skos:prefLabel "Cinerama"@en .

<http://rdaregistry.info/termList/presFormat/1002>
    rdakit:toolkitDefinition "A presentation format of a motion picture film that presents an aspect ratio of 2.59:1 using three synchronized projectors."@en ;
    rdakit:toolkitLabel "Cinemiracle"@en ;
    reg:identifier <http://metadataregistry.org/concepts/888> ;
    reg:status <http://metadataregistry.org/uri/RegStatus/1001> ;
    a skos:Concept ;
    skos:definition "A presentation format of a motion picture film that presents an aspect ratio of 2.59:1 using three synchronized projectors."@en ;
    skos:inScheme <http://rdaregistry.info/termList/presFormat> ;
    skos:prefLabel "Cinemiracle"@en .

<http://rdaregistry.info/termList/presFormat/1003>
    rdakit:toolkitDefinition "A presentation format of a motion picture film that uses nine projectors for screens arranged in a circle."@en ;
    rdakit:toolkitLabel "Circarama"@en ;
    reg:identifier <http://metadataregistry.org/concepts/889> ;
    reg:status <http://metadataregistry.org/uri/RegStatus/1001> ;
    a skos:Concept ;
    skos:altLabel "Circle-Vision"@en ;
    skos:definition "A presentation format of a motion picture film that uses nine projectors for screens arranged in a circle."@en ;
    skos:inScheme <http://rdaregistry.info/termList/presFormat> ;
    skos:prefLabel "Circarama"@en .

<http://rdaregistry.info/termList/presFormat/1004>
    rdakit:toolkitDefinition "A presentation format of a motion picture film that projects images of far greater size and resolution than conventional film systems."@en ;
    rdakit:toolkitLabel "IMAX"@en ;
    reg:identifier <http://metadataregistry.org/concepts/890> ;
    reg:status <http://metadataregistry.org/uri/RegStatus/1001> ;
    a skos:Concept ;
    skos:definition "A presentation format of a motion picture film that projects images of far greater size and resolution than conventional film systems."@en ;
    skos:inScheme <http://rdaregistry.info/termList/presFormat> ;
    skos:prefLabel "IMAX"@en .

<http://rdaregistry.info/termList/presFormat/1005>
    rdakit:toolkitDefinition "A presentation format of a motion picture film using multiple synchronized projectors."@en ;
    rdakit:toolkitLabel "multiprojector"@en ;
    reg:identifier <http://metadataregistry.org/concepts/891> ;
    reg:status <http://metadataregistry.org/uri/RegStatus/1001> ;
    a skos:Concept ;
    skos:definition "A presentation format of a motion picture film using multiple synchronized projectors."@en ;
    skos:inScheme <http://rdaregistry.info/termList/presFormat> ;
    skos:prefLabel "multiprojector"@en .

<http://rdaregistry.info/termList/presFormat/1006>
    rdakit:toolkitDefinition "A presentation format of a motion picture film using multiple screens."@en ;
    rdakit:toolkitLabel "multiscreen"@en ;
    reg:identifier <http://metadataregistry.org/concepts/892> ;
    reg:status <http://metadataregistry.org/uri/RegStatus/1001> ;
    a skos:Concept ;
    skos:definition "A presentation format of a motion picture film using multiple screens."@en ;
    skos:inScheme <http://rdaregistry.info/termList/presFormat> ;
    skos:prefLabel "multiscreen"@en .

<http://rdaregistry.info/termList/presFormat/1007>
    rdakit:toolkitDefinition "A presentation format of a motion picture film that presents a wide-screen aspect ratio using Panavision anamorphic lenses."@en ;
    rdakit:toolkitLabel "Panavision"@en ;
    reg:identifier <http://metadataregistry.org/concepts/893> ;
    reg:status <http://metadataregistry.org/uri/RegStatus/1001> ;
    a skos:Concept ;
    skos:definition "A presentation format of a motion picture film that presents a wide-screen aspect ratio using Panavision anamorphic lenses."@en ;
    skos:inScheme <http://rdaregistry.info/termList/presFormat> ;
    skos:prefLabel "Panavision"@en .

<http://rdaregistry.info/termList/presFormat/1008>
    rdakit:toolkitDefinition "A presentation format of a motion picture film that uses a standard projector aperture for silent film."@en ;
    rdakit:toolkitLabel "standard silent aperture"@en ;
    reg:identifier <http://metadataregistry.org/concepts/894> ;
    reg:status <http://metadataregistry.org/uri/RegStatus/1001> ;
    a skos:Concept ;
    skos:definition "A presentation format of a motion picture film that uses a standard projector aperture for silent film."@en ;
    skos:inScheme <http://rdaregistry.info/termList/presFormat> ;
    skos:prefLabel "standard silent aperture"@en .

<http://rdaregistry.info/termList/presFormat/1009>
    rdakit:toolkitDefinition "A presentation format of a motion picture film that uses a standard projector aperture for film with a sound-track."@en ;
    rdakit:toolkitLabel "standard sound aperture"@en ;
    reg:identifier <http://metadataregistry.org/concepts/895> ;
    reg:status <http://metadataregistry.org/uri/RegStatus/1001> ;
    a skos:Concept ;
    skos:definition "A presentation format of a motion picture film that uses a standard projector aperture for film with a sound-track."@en ;
    skos:inScheme <http://rdaregistry.info/termList/presFormat> ;
    skos:prefLabel "standard sound aperture"@en .

<http://rdaregistry.info/termList/presFormat/1010>
    rdakit:toolkitDefinition "A presentation format of a motion picture film that gives the illusion of three dimensions by using stereoscopic images."@en ;
    rdakit:toolkitLabel "stereoscopic"@en ;
    reg:identifier <http://metadataregistry.org/concepts/896> ;
    reg:status <http://metadataregistry.org/uri/RegStatus/1001> ;
    a skos:Concept ;
    skos:definition "A presentation format of a motion picture film that gives the illusion of three dimensions by using stereoscopic images."@en ;
    skos:inScheme <http://rdaregistry.info/termList/presFormat> ;
    skos:prefLabel "stereoscopic"@en .

<http://rdaregistry.info/termList/presFormat/1011>
    rdakit:toolkitDefinition "A presentation format of a motion picture film that presents an aspect ratio of 2.33:1 using 35 mm film."@en ;
    rdakit:toolkitLabel "Techniscope"@en ;
    reg:identifier <http://metadataregistry.org/concepts/897> ;
    reg:status <http://metadataregistry.org/uri/RegStatus/1001> ;
    a skos:Concept ;
    skos:definition "A presentation format of a motion picture film that presents an aspect ratio of 2.33:1 using 35 mm film."@en ;
    skos:inScheme <http://rdaregistry.info/termList/presFormat> ;
    skos:prefLabel "Techniscope"@en .

<http://rdaregistry.info/termList/presFormat/1012>
    rdakit:toolkitDefinition "A presentation format of a motion picture film that gives the illusion of three dimensions."@en ;
    rdakit:toolkitLabel "3D"@en ;
    reg:identifier <http://metadataregistry.org/concepts/898> ;
    reg:status <http://metadataregistry.org/uri/RegStatus/1001> ;
    a skos:Concept ;
    skos:definition "A presentation format of a motion picture film that gives the illusion of three dimensions."@en ;
    skos:inScheme <http://rdaregistry.info/termList/presFormat> ;
    skos:prefLabel "3D"@en .

