@prefix rdf: <http://www.w3.org/1999/02/22-rdf-syntax-ns#> .
@prefix dc: <http://purl.org/dc/elements/1.1/> .
@prefix reg: <http://metadataregistry.org/uri/profile/regap/> .
@prefix skos: <http://www.w3.org/2004/02/skos/core#> .

<http://metadataregistry.org/uri/RegStatus/1008>
    a skos:Concept ;
    skos:prefLabel "Deprecated"@en .

<http://rdaregistry.info/termList/prodManuscript>
    dc:title "RDA Production Method for Manuscript (Deprecated)" ;
    a skos:ConceptScheme .

<http://rdaregistry.info/termList/prodManuscript/1001>
    reg:identifier <http://metadataregistry.org/concepts/807> ;
    reg:status <http://metadataregistry.org/uri/RegStatus/1008> ;
    a skos:Concept ;
    skos:definition "A manuscript handwritten by the person or persons responsible for the work or works contained therein. (Deprecated)"@en ;
    skos:inScheme <http://rdaregistry.info/termList/prodManuscript> ;
    skos:prefLabel "holograph (Deprecated)"@en .

<http://rdaregistry.info/termList/prodManuscript/1002>
    reg:identifier <http://metadataregistry.org/concepts/808> ;
    reg:status <http://metadataregistry.org/uri/RegStatus/1008> ;
    a skos:Concept ;
    skos:definition "In the context of production method for manuscripts, any handwritten manuscript which is not a holograph. (Deprecated)"@en ;
    skos:inScheme <http://rdaregistry.info/termList/prodManuscript> ;
    skos:prefLabel "manuscript (Deprecated)"@en .

<http://rdaregistry.info/termList/prodManuscript/1003>
    reg:identifier <http://metadataregistry.org/concepts/809> ;
    reg:status <http://metadataregistry.org/uri/RegStatus/1008> ;
    a skos:Concept ;
    skos:definition "Text, images or other data from a computer file printed as output on paper, or some other printing surface, by a peripheral device (a printer). (Deprecated)"@en ;
    skos:inScheme <http://rdaregistry.info/termList/prodManuscript> ;
    skos:prefLabel "printout (Deprecated)"@en .

<http://rdaregistry.info/termList/prodManuscript/1004>
    reg:identifier <http://metadataregistry.org/concepts/810> ;
    reg:status <http://metadataregistry.org/uri/RegStatus/1008> ;
    a skos:Concept ;
    skos:altLabel "Typescript (Deprecated)"@en ;
    skos:inScheme <http://rdaregistry.info/termList/prodManuscript> ;
    skos:prefLabel "typewritten (Deprecated)"@en .

<http://rdaregistry.info/termList/prodManuscript/1005>
    reg:identifier <http://metadataregistry.org/concepts/1105> ;
    reg:status <http://metadataregistry.org/uri/RegStatus/1008> ;
    a skos:Concept ;
    skos:definition "A production method for manuscript that uses an intermediate sheet of paper coated with carbon to create copies at the same time as the original. (Deprecated)"@en ;
    skos:inScheme <http://rdaregistry.info/termList/prodManuscript> ;
    skos:prefLabel "carbon copy (Deprecated)"@en .

<http://rdaregistry.info/termList/prodManuscript/1006>
    reg:identifier <http://metadataregistry.org/concepts/1106> ;
    reg:status <http://metadataregistry.org/uri/RegStatus/1008> ;
    a skos:Concept ;
    skos:definition "A macroform photoreproduction produced directly on opaque material by radiant energy through contact or projection. (Deprecated)"@en ;
    skos:inScheme <http://rdaregistry.info/termList/prodManuscript> ;
    skos:prefLabel "photocopy (Deprecated)"@en .

<http://rdaregistry.info/termList/prodManuscript/1007>
    reg:identifier <http://metadataregistry.org/concepts/1107> ;
    reg:status <http://metadataregistry.org/uri/RegStatus/1008> ;
    a skos:Concept ;
    skos:definition "A copy of an original, usually made by hand or typewritten (e.g., a legal document, an official record). (Deprecated)"@en ;
    skos:inScheme <http://rdaregistry.info/termList/prodManuscript> ;
    skos:prefLabel "transcript (Deprecated)"@en .

<http://rdaregistry.info/termList/prodManuscript/1008>
    reg:identifier <http://metadataregistry.org/concepts/1108> ;
    reg:status <http://metadataregistry.org/uri/RegStatus/1008> ;
    a skos:Concept ;
    skos:inScheme <http://rdaregistry.info/termList/prodManuscript> ;
    skos:prefLabel "handwritten (Deprecated)"@en .

<http://rdaregistry.info/termList/prodManuscript/1009>
    reg:identifier <http://metadataregistry.org/concepts/3391> ;
    reg:status <http://metadataregistry.org/uri/RegStatus/1008> ;
    a skos:Concept ;
    skos:definition "A creatorâ€™s original typewritten copy of a work or a typewritten copy of the original commissioned by a creator or publisher, as opposed to a manuscript written by hand. (Deprecated)"@en ;
    skos:inScheme <http://rdaregistry.info/termList/prodManuscript> ;
    skos:prefLabel "typescript (Deprecated)"@en .

