@prefix rdf: <http://www.w3.org/1999/02/22-rdf-syntax-ns#> .
@prefix dc: <http://purl.org/dc/elements/1.1/> .
@prefix rdakit: <http://metadataregistry.org/uri/profile/rdakit/> .
@prefix reg: <http://metadataregistry.org/uri/profile/regap/> .
@prefix skos: <http://www.w3.org/2004/02/skos/core#> .

<http://metadataregistry.org/uri/RegStatus/1001>
    a skos:Concept ;
    skos:prefLabel "Published"@en .

<http://rdaregistry.info/termList/RDACartoDT>
    dc:title "RDA Cartographic Data Type" ;
    a skos:ConceptScheme .

<http://rdaregistry.info/termList/RDACartoDT/1001>
    rdakit:toolkitDefinition "A cartographic data type that uses a dot matrix data structure to represent features in a usually rectangular grid of pixels."@en ;
    rdakit:toolkitLabel "Raster"@de, "raster"@en, "raster"@es, "raster"@it, "rasteri"@fi, "trame"@fr ;
    reg:identifier <http://metadataregistry.org/concepts/8503> ;
    reg:status <http://metadataregistry.org/uri/RegStatus/1001> ;
    a skos:Concept ;
    skos:definition "A cartographic data type that uses a dot matrix data structure to represent features in a usually rectangular grid of pixels."@en ;
    skos:inScheme <http://rdaregistry.info/termList/RDACartoDT> ;
    skos:prefLabel "Raster"@de, "raster"@en, "raster"@es, "raster"@it, "rasteri"@fi, "trame"@fr .

<http://rdaregistry.info/termList/RDACartoDT/1002>
    rdakit:toolkitDefinition "A cartographic data type that uses polygons specified by vectors to represent features."@en ;
    rdakit:toolkitLabel "Vektor"@de, "vecteur"@fr, "vector"@en, "vector"@es, "vektori"@fi, "vettore"@it ;
    reg:identifier <http://metadataregistry.org/concepts/8504> ;
    reg:status <http://metadataregistry.org/uri/RegStatus/1001> ;
    a skos:Concept ;
    skos:definition "A cartographic data type that uses polygons specified by vectors to represent features."@en ;
    skos:inScheme <http://rdaregistry.info/termList/RDACartoDT> ;
    skos:prefLabel "Vektor"@de, "vecteur"@fr, "vector"@en, "vector"@es, "vektori"@fi, "vettore"@it .

<http://rdaregistry.info/termList/RDACartoDT/1003>
    rdakit:toolkitDefinition "A cartographic data type that uses points to represent features."@en ;
    rdakit:toolkitLabel "Punkt"@de, "piste"@fi, "point"@en, "point"@fr, "punto"@es, "punto"@it ;
    reg:identifier <http://metadataregistry.org/concepts/8505> ;
    reg:status <http://metadataregistry.org/uri/RegStatus/1001> ;
    a skos:Concept ;
    skos:definition "A cartographic data type that uses points to represent features."@en ;
    skos:inScheme <http://rdaregistry.info/termList/RDACartoDT> ;
    skos:prefLabel "Punkt"@de, "piste"@fi, "point"@en, "point"@fr, "punto"@es, "punto"@it .

