@prefix rdf: <http://www.w3.org/1999/02/22-rdf-syntax-ns#> .
@prefix dc: <http://purl.org/dc/elements/1.1/> .
@prefix rdakit: <http://metadataregistry.org/uri/profile/rdakit/> .
@prefix reg: <http://metadataregistry.org/uri/profile/regap/> .
@prefix skos: <http://www.w3.org/2004/02/skos/core#> .

<http://metadataregistry.org/uri/RegStatus/1001>
    a skos:Concept ;
    skos:prefLabel "Published"@en .

<http://rdaregistry.info/termList/RDATerms>
    dc:title "RDA Terms" ;
    a skos:ConceptScheme .

<http://rdaregistry.info/termList/RDATerms/1001>
    rdakit:toolkitDefinition "A name, term, code, etc., representing a specific entity."@en, "Nom, terme, code, etc. représentant une entité spécifique."@fr, "Nombre, término, código, etc., bajo el cual podrá encontrarse información que pertenece a una entidad específica."@es, "Nome, termine, codice, etc. che rappresenta un'entità specifica."@it ;
    rdakit:toolkitLabel "access point"@en, "point d’accès"@fr, "punto d'accesso"@it, "punto de acceso"@es ;
    reg:identifier <http://metadataregistry.org/concepts/8516> ;
    reg:status <http://metadataregistry.org/uri/RegStatus/1001> ;
    a skos:Concept ;
    skos:definition "A name, term, code, etc., representing a specific entity."@en, "Nom, terme, code, etc. représentant une entité spécifique."@fr, "Nombre, término, código, etc., bajo el cual podrá encontrarse información que pertenece a una entidad específica."@es, "Nome, termine, codice, etc. che rappresenta un'entità specifica."@it ;
    skos:inScheme <http://rdaregistry.info/termList/RDATerms> ;
    skos:narrower <http://rdaregistry.info/termList/RDATerms/1012>, <http://rdaregistry.info/termList/RDATerms/1102> ;
    skos:prefLabel "access point"@en, "point d’accès"@fr, "punto d'accesso"@it, "punto de acceso"@es .

<http://rdaregistry.info/termList/RDATerms/1002>
    rdakit:toolkitDefinition "An accessible tactile language text that is attached to a tactile image, map or diagram."@en, "Testo linguistico accessibile al tatto, presente su un'immagine, carta geografica o diagramma tattile."@it ;
    rdakit:toolkitLabel "accessible labels"@en, "etichette accessibili"@it ;
    reg:identifier <http://metadataregistry.org/concepts/8517> ;
    reg:status <http://metadataregistry.org/uri/RegStatus/1001> ;
    a skos:Concept ;
    skos:definition "An accessible tactile language text that is attached to a tactile image, map or diagram."@en, "Testo linguistico accessibile al tatto, presente su un'immagine, carta geografica o diagramma tattile."@it ;
    skos:inScheme <http://rdaregistry.info/termList/RDATerms> ;
    skos:prefLabel "accessible labels"@en, "etichette accessibili"@it .

<http://rdaregistry.info/termList/RDATerms/1003>
    rdakit:toolkitDefinition "A new derivative work created by revision of a previously existing work that substantially changes the nature and content of that work."@en, "Nouvelle œuvre dérivée créée par la révision d’une œuvre préexistante qui change considérablement la nature et le contenu de cette œuvre."@fr, "Nuova opera derivata, nata dalla revisione di un'opera preesistente, che ne modifica sostanzialmente natura e contenuto."@it ;
    rdakit:toolkitLabel "adaptation"@en, "adaptation"@fr, "adattamento"@it ;
    reg:identifier <http://metadataregistry.org/concepts/8518> ;
    reg:status <http://metadataregistry.org/uri/RegStatus/1001> ;
    a skos:Concept ;
    skos:definition "A new derivative work created by revision of a previously existing work that substantially changes the nature and content of that work."@en, "Nouvelle œuvre dérivée créée par la révision d’une œuvre préexistante qui change considérablement la nature et le contenu de cette œuvre."@fr, "Nuova opera derivata, nata dalla revisione di un'opera preesistente, che ne modifica sostanzialmente natura e contenuto."@it ;
    skos:inScheme <http://rdaregistry.info/termList/RDATerms> ;
    skos:prefLabel "adaptation"@en, "adaptation"@fr, "adattamento"@it ;
    skos:related <http://rdaregistry.info/termList/RDATerms/1008> ;
    skos:scopeNote "In the case of a musical work, a derivative work described as freely transcribed, based on, etc.; a revision incorporating new material; a paraphrase of various works by, or in the general style of, another composer; revisions in which the harmony or musical style of the original has been changed; performances involving substantial creative responsibility for adaptation, improvisation, etc., on the part of the performer or performers; or any other distinct alteration of another musical work, are included."@en .

<http://rdaregistry.info/termList/RDATerms/1004>
    rdakit:toolkitDefinition "A title page preceding or following the title page chosen as the preferred source of information."@en, "Frontespizio che precede o segue il frontespizio scelto come fonte d'informazione preferita."@it ;
    rdakit:toolkitLabel "added title page"@en, "frontespizio aggiunto"@it ;
    reg:identifier <http://metadataregistry.org/concepts/8519> ;
    reg:status <http://metadataregistry.org/uri/RegStatus/1001> ;
    a skos:Concept ;
    skos:definition "A title page preceding or following the title page chosen as the preferred source of information."@en, "Frontespizio che precede o segue il frontespizio scelto come fonte d'informazione preferita."@it ;
    skos:inScheme <http://rdaregistry.info/termList/RDATerms> ;
    skos:prefLabel "added title page"@en, "frontespizio aggiunto"@it ;
    skos:related <http://rdaregistry.info/termList/RDATerms/1082>, <http://rdaregistry.info/termList/RDATerms/1095> ;
    skos:scopeNote "An added title page may be more general or equally general. A series title page is an example of a more general title page; a title page is another language is an example of an equally general title page."@en, "Può essere di livello superiore (per esempio, un frontespizio della serie) o dello stesso livello (per esempio, un frontespizio in un'altra lingua)."@it .

<http://rdaregistry.info/termList/RDATerms/1005>
    rdakit:toolkitDefinition "A second part of a title proper that consists of two parts, each of which has the form of an independent title, joined by a word such as \"or\" or its equivalent in another language."@en, "La seconde partie d’un titre propre composé de deux parties (dont chacune se présente comme un titre indépendant) reliées par un mot tel que « ou » ou son équivalent dans une autre langue."@fr, "Seconda parte di un titolo proprio che consiste di due parti (ciascuna delle quali ha la forma di un titolo indipendente), unite da una congiunzione come o o da un suo equivalente in altra lingua."@it, "Segunda parte de un título propiamente dicho que consiste en dos partes (cada una de las cuales tiene la forma de un título independiente), unida mediante una palabra tal como \"o\" o su equivalente en otra lengua."@es ;
    rdakit:toolkitLabel "alternative title"@en, "titolo alternativo"@it, "titre alternatif"@fr, "título alternativo"@es ;
    reg:identifier <http://metadataregistry.org/concepts/8520> ;
    reg:status <http://metadataregistry.org/uri/RegStatus/1001> ;
    a skos:Concept ;
    skos:definition "A second part of a title proper that consists of two parts, each of which has the form of an independent title, joined by a word such as \"or\" or its equivalent in another language."@en, "La seconde partie d’un titre propre composé de deux parties (dont chacune se présente comme un titre indépendant) reliées par un mot tel que « ou » ou son équivalent dans une autre langue."@fr, "Seconda parte di un titolo proprio che consiste di due parti (ciascuna delle quali ha la forma di un titolo indipendente), unite da una congiunzione come o o da un suo equivalente in altra lingua."@it, "Segunda parte de un título propiamente dicho que consiste en dos partes (cada una de las cuales tiene la forma de un título independiente), unida mediante una palabra tal como \"o\" o su equivalente en otra lengua."@es ;
    skos:inScheme <http://rdaregistry.info/termList/RDATerms> ;
    skos:prefLabel "alternative title"@en, "titolo alternativo"@it, "titre alternatif"@fr, "título alternativo"@es .

<http://rdaregistry.info/termList/RDATerms/1006>
    rdakit:toolkitDefinition "A description that describes a part of a larger manifestation."@en, "Descripción que describe una parte de un recurso mayor."@es, "Description d’une partie d’une ressource plus vaste."@fr, "Descrizione di una parte di una risorsa più ampia"@it ;
    rdakit:toolkitLabel "analytical description"@en, "descripción analítica"@es, "description analytique"@fr, "descrizione analitica"@it ;
    reg:identifier <http://metadataregistry.org/concepts/8521> ;
    reg:status <http://metadataregistry.org/uri/RegStatus/1001> ;
    a skos:Concept ;
    skos:definition "A description that describes a part of a larger manifestation."@en, "Descripción que describe una parte de un recurso mayor."@es, "Description d’une partie d’une ressource plus vaste."@fr, "Descrizione di una parte di una risorsa più ampia"@it ;
    skos:inScheme <http://rdaregistry.info/termList/RDATerms> ;
    skos:prefLabel "analytical description"@en, "descripción analítica"@es, "description analytique"@fr, "descrizione analitica"@it ;
    skos:scopeNote "Analytical description includes a description for a single volume of a three-volume biography, a single map forming part of a map series, etc."@en .

<http://rdaregistry.info/termList/RDATerms/1007>
    rdakit:toolkitDefinition "A document or documents organically created, accumulated, or used by an agent in the course of the conduct of affairs and preserved because of their continuing value."@en, "Document ou ensemble de documents organiquement créé, accumulé, et/ou utilisé par une personne, famille ou collectivité au cours de son activité et préservé en raison de sa valeur constante."@fr, "Documento o documenti creati, accumulati e/o utilizzati organicamente da una persona, famiglia, ente nella conduzione delle proprie attività e conservati per il loro valore permanente."@it, "Documento o documentos creados orgánicamente, acumulados y/o usados por una persona, familia o entidad corporativa en el curso de la gestión de sus asuntos; y preservada debido a su valor duradero."@es ;
    rdakit:toolkitLabel "archival resource"@en, "recurso archivítico"@es, "ressource archivistique"@fr, "risorsa archivistica"@it ;
    reg:identifier <http://metadataregistry.org/concepts/8522> ;
    reg:status <http://metadataregistry.org/uri/RegStatus/1001> ;
    a skos:Concept ;
    skos:definition "A document or documents organically created, accumulated, or used by an agent in the course of the conduct of affairs and preserved because of their continuing value."@en, "Document ou ensemble de documents organiquement créé, accumulé, et/ou utilisé par une personne, famille ou collectivité au cours de son activité et préservé en raison de sa valeur constante."@fr, "Documento o documenti creati, accumulati e/o utilizzati organicamente da una persona, famiglia, ente nella conduzione delle proprie attività e conservati per il loro valore permanente."@it, "Documento o documentos creados orgánicamente, acumulados y/o usados por una persona, familia o entidad corporativa en el curso de la gestión de sus asuntos; y preservada debido a su valor duradero."@es ;
    skos:inScheme <http://rdaregistry.info/termList/RDATerms> ;
    skos:prefLabel "archival resource"@en, "recurso archivítico"@es, "ressource archivistique"@fr, "risorsa archivistica"@it ;
    skos:scopeNote "Cette ressource peut être aussi bien une agrégation de documents qu’un item isolé. Elle peut être également une collection acquise et rassemblée par un dépôt d’archives, un particulier, une autre institution et qui n’a ni provenance ni origine communes mais qui présente des caractéristiques communes, comme un sujet, un thème ou une forme spécifiques."@fr, "Este recurso puede ser una agregación de documentos o puede ser un ítem separado. También puede ser una colección adquirida y reunida por un repositorio de archivo, un individuo u otra institución, que no comparte un origen o procedencia común pero que refleja alguna característica común, por ejemplo, un tema, una materia o una forma determinadas."@es, "Questa risorsa può essere un'aggregazione di documenti o può essere un item distinto. Può essere anche una collezione acquisita e assemblata da un archivio, individuo o altra istituzione, che non ha una provenienza o un'origine comune ma condivide qualche caratteristica comune, per esempio, un soggetto, un tema o una forma particolari."@it, "The resource may be an aggregation of documents or it may be a discrete item. It may also be a collection acquired and assembled by an archival repository, individual, or other institution, that does not share a common provenance or origin but that reflects some common characteristic, for example, a particular subject, theme, or form."@en .

<http://rdaregistry.info/termList/RDATerms/1008>
    rdakit:toolkitDefinition "An expression of a musical work resulting either from a change in the medium of performance, or from a simplification or other modification of the work with or without a change in medium of performance."@en, "Espressione di un'opera musicale che risulta da (a) un cambiamento nel mezzo d’interpretazione o (b) una semplificazione o altra modifica dell'opera, con o senza cambiamento del mezzo d’interpretazione."@it ;
    rdakit:toolkitLabel "arrangement"@en ;
    reg:identifier <http://metadataregistry.org/concepts/8523> ;
    reg:status <http://metadataregistry.org/uri/RegStatus/1001> ;
    a skos:Concept ;
    skos:definition "An expression of a musical work resulting either from a change in the medium of performance, or from a simplification or other modification of the work with or without a change in medium of performance."@en, "Espressione di un'opera musicale che risulta da (a) un cambiamento nel mezzo d’interpretazione o (b) una semplificazione o altra modifica dell'opera, con o senza cambiamento del mezzo d’interpretazione."@it ;
    skos:inScheme <http://rdaregistry.info/termList/RDATerms> ;
    skos:prefLabel "arrangement"@en ;
    skos:related <http://rdaregistry.info/termList/RDATerms/1003> .

<http://rdaregistry.info/termList/RDATerms/1009>
    rdakit:toolkitDefinition "A narrative text, read out loud by a human being or by voice synthesis, that succinctly explains visual details not apparent from the audio element of the expression."@en, "Testo narrativo, letto ad alta voce da un essere umano o da una voce sintetica, che spiega in sintesi i dettagli visivi non evidenti dall'elemento audio della risorsa."@it, "Texte descriptif, lu à haute voix par un être humain ou par une voix de synthèse, qui explique succinctement des détails visuels dont l’élément audio de la ressource ne rend pas compte."@fr ;
    rdakit:toolkitLabel "audio description"@en, "description audio"@fr, "descrizione audio"@it ;
    reg:identifier <http://metadataregistry.org/concepts/8524> ;
    reg:status <http://metadataregistry.org/uri/RegStatus/1001> ;
    a skos:Concept ;
    skos:altLabel "audio captioning"@en, "intitolazione audio"@it ;
    skos:definition "A narrative text, read out loud by a human being or by voice synthesis, that succinctly explains visual details not apparent from the audio element of the expression."@en, "Testo narrativo, letto ad alta voce da un essere umano o da una voce sintetica, che spiega in sintesi i dettagli visivi non evidenti dall'elemento audio della risorsa."@it, "Texte descriptif, lu à haute voix par un être humain ou par une voix de synthèse, qui explique succinctement des détails visuels dont l’élément audio de la ressource ne rend pas compte."@fr ;
    skos:inScheme <http://rdaregistry.info/termList/RDATerms> ;
    skos:prefLabel "audio description"@en, "description audio"@fr, "descrizione audio"@it .

<http://rdaregistry.info/termList/RDATerms/1010>
    rdakit:toolkitDefinition "A recording on which sound vibrations have been registered by mechanical or electrical means so that the sound may be reproduced."@en, "Registrazione in cui le vibrazioni sonore sono state registrate per mezzo di strumenti meccanici o elettrici in modo che il suono possa essere riprodotto."@it ;
    rdakit:toolkitLabel "audio recording"@en, "registrazione audio"@it ;
    reg:identifier <http://metadataregistry.org/concepts/8525> ;
    reg:status <http://metadataregistry.org/uri/RegStatus/1001> ;
    a skos:Concept ;
    skos:definition "A recording on which sound vibrations have been registered by mechanical or electrical means so that the sound may be reproduced."@en, "Registrazione in cui le vibrazioni sonore sono state registrate per mezzo di strumenti meccanici o elettrici in modo che il suono possa essere riprodotto."@it ;
    skos:inScheme <http://rdaregistry.info/termList/RDATerms> ;
    skos:prefLabel "audio recording"@en, "registrazione audio"@it .

<http://rdaregistry.info/termList/RDATerms/1011>
    rdakit:toolkitDefinition "A length of magnetic tape on which are recorded electrical signals that can be converted to sound using audio playback equipment."@en, "Métrage de bande magnétique sur laquelle sont enregistrés des signaux électriques qui peuvent être convertis en sons à l’aide d’un appareil de lecture."@fr, "Striscia di nastro magnetico sulla quale sono registrati segnali elettrici che possono essere convertiti in suono utilizzando un’attrezzatura per la riproduzione audio."@it ;
    rdakit:toolkitLabel "audiotape"@en, "bande audio"@fr, "nastro audio"@it ;
    reg:identifier <http://metadataregistry.org/concepts/8526> ;
    reg:status <http://metadataregistry.org/uri/RegStatus/1001> ;
    a skos:Concept ;
    skos:definition "A length of magnetic tape on which are recorded electrical signals that can be converted to sound using audio playback equipment."@en, "Métrage de bande magnétique sur laquelle sont enregistrés des signaux électriques qui peuvent être convertis en sons à l’aide d’un appareil de lecture."@fr, "Striscia di nastro magnetico sulla quale sono registrati segnali elettrici che possono essere convertiti in suono utilizzando un’attrezzatura per la riproduzione audio."@it ;
    skos:inScheme <http://rdaregistry.info/termList/RDATerms> ;
    skos:prefLabel "audiotape"@en, "bande audio"@fr, "nastro audio"@it .

<http://rdaregistry.info/termList/RDATerms/1012>
    rdakit:toolkitDefinition "A standardized access point representing an entity."@en, "Entiteetin vahvistettu hakutieto."@fi, "Le point d’accès normalisé représentant une entité."@fr, "Punto d'accesso standardizzato che rappresenta un'entità."@it, "Punto de acceso normalizado que representa una entidad."@es ;
    rdakit:toolkitLabel "auktorisoitu hakutieto"@fi, "authorized access point"@en, "point d’accès autorisé"@fr, "punto d'accesso autorizzato"@it, "punto de acceso autorizado"@es ;
    reg:identifier <http://metadataregistry.org/concepts/8527> ;
    reg:status <http://metadataregistry.org/uri/RegStatus/1001> ;
    a skos:Concept ;
    skos:broader <http://rdaregistry.info/termList/RDATerms/1001> ;
    skos:definition "A standardized access point representing an entity."@en, "Entiteetin vahvistettu hakutieto."@fi, "Le point d’accès normalisé représentant une entité."@fr, "Punto d'accesso standardizzato che rappresenta un'entità."@it, "Punto de acceso normalizado que representa una entidad."@es ;
    skos:inScheme <http://rdaregistry.info/termList/RDATerms> ;
    skos:prefLabel "auktorisoitu hakutieto"@fi, "authorized access point"@en, "point d’accès autorisé"@fr, "punto d'accesso autorizzato"@it, "punto de acceso autorizado"@es .

<http://rdaregistry.info/termList/RDATerms/1013>
    rdakit:toolkitDefinition "An outer cover affixed to a gathering of one or more sheets."@en, "Copertura esterna apposta a un fascicolo di uno o più fogli."@it, "Couverture extérieure fixée à un cahier d’une ou plusieurs feuilles."@fr ;
    rdakit:toolkitLabel "binding"@en, "legatura"@it, "reliure"@fr ;
    reg:identifier <http://metadataregistry.org/concepts/8528> ;
    reg:status <http://metadataregistry.org/uri/RegStatus/1001> ;
    a skos:Concept ;
    skos:definition "An outer cover affixed to a gathering of one or more sheets."@en, "Copertura esterna apposta a un fascicolo di uno o più fogli."@it, "Couverture extérieure fixée à un cahier d’une ou plusieurs feuilles."@fr ;
    skos:inScheme <http://rdaregistry.info/termList/RDATerms> ;
    skos:prefLabel "binding"@en, "legatura"@it, "reliure"@fr .

<http://rdaregistry.info/termList/RDATerms/1014>
    rdakit:toolkitDefinition "A title given at the beginning of the first page of the text or, for notated music, at the top of the first page."@en, "Titolo che figura all'inizio della prima pagina di testo o, per la musica notata, alla sommità della prima pagina."@it ;
    rdakit:toolkitLabel "caption title"@en, "intitolazione"@it ;
    reg:identifier <http://metadataregistry.org/concepts/8529> ;
    reg:status <http://metadataregistry.org/uri/RegStatus/1001> ;
    a skos:Concept ;
    skos:definition "A title given at the beginning of the first page of the text or, for notated music, at the top of the first page."@en, "Titolo che figura all'inizio della prima pagina di testo o, per la musica notata, alla sommità della prima pagina."@it ;
    skos:inScheme <http://rdaregistry.info/termList/RDATerms> ;
    skos:prefLabel "caption title"@en, "intitolazione"@it .

<http://rdaregistry.info/termList/RDATerms/1015>
    rdakit:toolkitDefinition "A text representing speech and other audible information that is displayed on screen in the written language of the audio element of the expression."@en, "Testo che rappresenta il parlato e altre informazioni in forma sonora e che è visualizzato sullo schermo nella lingua dell'elemento audio della risorsa."@it ;
    rdakit:toolkitLabel "captioning"@en, "didascalia"@it ;
    reg:identifier <http://metadataregistry.org/concepts/8530> ;
    reg:status <http://metadataregistry.org/uri/RegStatus/1001> ;
    a skos:Concept ;
    skos:definition "A text representing speech and other audible information that is displayed on screen in the written language of the audio element of the expression."@en, "Testo che rappresenta il parlato e altre informazioni in forma sonora e che è visualizzato sullo schermo nella lingua dell'elemento audio della risorsa."@it ;
    skos:inScheme <http://rdaregistry.info/termList/RDATerms> ;
    skos:prefLabel "captioning"@en, "didascalia"@it ;
    skos:scopeNote "Solitamente presente come \"didascalia nascosta\" codificata che deve essere decodificata (o attivata) per essere resa visibile. Esistono anche le \"didascalie in chiaro\" che sono sempre visibili e che non possono essere disattivate. Sono esclusi i sottotitoli in lingue diverse dal contenuto parlato."@it, "This is usually found as closed captions that are encoded and must be decoded, that is,  switched on, to be made visible. There are also open captions which are always visible and cannot be turned off. Excludes subtitles in a language different from the spoken content."@en .

<http://rdaregistry.info/termList/RDATerms/1016>
    rdakit:toolkitDefinition "A physical medium in which data, sound, images, etc., are stored."@en, "Mezzo fisico in cui si memorizzano dati, suoni, immagini, etc."@it, "Support physique sur lequel des données, du son, des images, etc. sont emmagasinés."@fr ;
    rdakit:toolkitLabel "carrier"@en, "support matériel"@fr, "supporto"@it ;
    reg:identifier <http://metadataregistry.org/concepts/8531> ;
    reg:status <http://metadataregistry.org/uri/RegStatus/1001> ;
    a skos:Concept ;
    skos:definition "A physical medium in which data, sound, images, etc., are stored."@en, "Mezzo fisico in cui si memorizzano dati, suoni, immagini, etc."@it, "Support physique sur lequel des données, du son, des images, etc. sont emmagasinés."@fr ;
    skos:inScheme <http://rdaregistry.info/termList/RDATerms> ;
    skos:prefLabel "carrier"@en, "support matériel"@fr, "supporto"@it ;
    skos:related <http://rdaregistry.info/termList/RDATerms/1026>, <http://rdaregistry.info/termList/RDATerms/1058>, <http://rdaregistry.info/termList/RDATerms/1086> ;
    skos:scopeNote "For certain types of manifestations, the carrier may consist of a storage medium  sometimes encased in a plastic, metal, etc., housing that is an integral part of the manifestation."@en, "Per alcuni tipi di risorsa, il supporto può consistere in un mezzo di memorizzazione (per esempio, nastro, pellicola) talvolta rivestito da una custodia di plastica, di metallo, etc. (per esempio, cassette, cartucce) che è parte integrante della risorsa."@it, "Pour certains types de ressources, le support matériel peut consister en un support de stockage (par exemple, une bande magnétique, un film) parfois intégré dans un contenant en plastique, en métal, etc. (par exemple, une cassette, une cartouche) qui fait partie intégrante de la ressource."@fr .

<http://rdaregistry.info/termList/RDATerms/1017>
    rdakit:toolkitDefinition "A content that represents the whole or part of the Earth, any celestial body, or imaginary place at any scale."@en, "Contenido que representa a toda o una parte de la Tierra, a los cuerpos celestes o lugares ficticios en cualquier escala."@es, "Contenu qui représente la totalité ou une partie de la Terre, tout corps céleste ou lieu imaginaire à n’importe quelle échelle."@fr, "Contenuto che rappresenta per intero o in parte la Terra, qualsiasi corpo celeste o luogo immaginario in qualunque scala."@it ;
    rdakit:toolkitLabel "cartographic content"@en, "contenido cartográfico"@es, "contenu cartographique"@fr, "contenuto cartografico"@it ;
    reg:identifier <http://metadataregistry.org/concepts/8532> ;
    reg:status <http://metadataregistry.org/uri/RegStatus/1001> ;
    a skos:Concept ;
    skos:definition "A content that represents the whole or part of the Earth, any celestial body, or imaginary place at any scale."@en, "Contenido que representa a toda o una parte de la Tierra, a los cuerpos celestes o lugares ficticios en cualquier escala."@es, "Contenu qui représente la totalité ou une partie de la Terre, tout corps céleste ou lieu imaginaire à n’importe quelle échelle."@fr, "Contenuto che rappresenta per intero o in parte la Terra, qualsiasi corpo celeste o luogo immaginario in qualunque scala."@it ;
    skos:inScheme <http://rdaregistry.info/termList/RDATerms> ;
    skos:prefLabel "cartographic content"@en, "contenido cartográfico"@es, "contenu cartographique"@fr, "contenuto cartografico"@it .

<http://rdaregistry.info/termList/RDATerms/1018>
    rdakit:toolkitDefinition "A title of a legal work used for the citation of the work either in the text of the work or in legal literature."@en, "Titolo di un'opera giuridica utilizzato per la citazione dell'opera nel testo dell'opera stessa o nella letteratura giuridica."@it, "Titre d’une œuvre juridique utilisé pour faire référence à l’œuvre, que ce soit dans le texte même de l’œuvre ou dans la littérature juridique."@fr, "Un título de una obra jurídica usado para citar la obra ya sea en el texto de la obra o en la literatura jurídica."@es ;
    rdakit:toolkitLabel "citation title of a legal work"@en, "titolo di citazione di un'opera giuridica"@it, "titre de référence d’une œuvre juridique"@fr, "título de citación de una obra jurídica"@es ;
    reg:identifier <http://metadataregistry.org/concepts/8533> ;
    reg:status <http://metadataregistry.org/uri/RegStatus/1001> ;
    a skos:Concept ;
    skos:definition "A title of a legal work used for the citation of the work either in the text of the work or in legal literature."@en, "Titolo di un'opera giuridica utilizzato per la citazione dell'opera nel testo dell'opera stessa o nella letteratura giuridica."@it, "Titre d’une œuvre juridique utilisé pour faire référence à l’œuvre, que ce soit dans le texte même de l’œuvre ou dans la littérature juridique."@fr, "Un título de una obra jurídica usado para citar la obra ya sea en el texto de la obra o en la literatura jurídica."@es ;
    skos:inScheme <http://rdaregistry.info/termList/RDATerms> ;
    skos:prefLabel "citation title of a legal work"@en, "titolo di citazione di un'opera giuridica"@it, "titre de référence d’une œuvre juridique"@fr, "título de citación de una obra jurídica"@es .

<http://rdaregistry.info/termList/RDATerms/1019>
    rdakit:toolkitDefinition "A group of resources assembled by an agent from a variety of sources."@en, "Groupe de ressources d’origine variée rassemblées par une personne, famille ou collectivité."@fr, "Grupo de recursos reunido, por una persona, familia o entidad corporativa, a partir de una variedad de fuentes."@es, "Gruppo di risorse riunite da una persona, famiglia o ente attingendo a una varietà di fonti."@it ;
    rdakit:toolkitLabel "colección"@es, "collection"@en, "collection"@fr, "collezione"@it ;
    reg:identifier <http://metadataregistry.org/concepts/8534> ;
    reg:status <http://metadataregistry.org/uri/RegStatus/1001> ;
    a skos:Concept ;
    skos:definition "A group of resources assembled by an agent from a variety of sources."@en, "Groupe de ressources d’origine variée rassemblées par une personne, famille ou collectivité."@fr, "Grupo de recursos reunido, por una persona, familia o entidad corporativa, a partir de una variedad de fuentes."@es, "Gruppo di risorse riunite da una persona, famiglia o ente attingendo a una varietà di fonti."@it ;
    skos:inScheme <http://rdaregistry.info/termList/RDATerms> ;
    skos:prefLabel "colección"@es, "collection"@en, "collection"@fr, "collezione"@it .

<http://rdaregistry.info/termList/RDATerms/1020>
    rdakit:toolkitDefinition "An inclusive title used either as a title proper for a manifestation containing separately titled individual contents, or as a preferred title for a compilation of two or more works."@en, "Titolo proprio che è un titolo comprensivo di una risorsa che contiene più parti componenti intitolate distintamente."@it, "Titre propre qui est un titre global pour une ressource contenant plusieurs parties composantes titrées séparément."@fr, "Título inclusivo usado ya sea como el título propiamente dicho para un recurso que tiene contenido individual titulado separadamente, o como el título preferido para una compilación de dos o más obra."@es ;
    rdakit:toolkitLabel "collective title"@en, "titolo collettivo"@it, "titre collectif"@fr, "título colectivo"@es ;
    reg:identifier <http://metadataregistry.org/concepts/8535> ;
    reg:status <http://metadataregistry.org/uri/RegStatus/1001> ;
    a skos:Concept ;
    skos:definition "An inclusive title used either as a title proper for a manifestation containing separately titled individual contents, or as a preferred title for a compilation of two or more works."@en, "Titolo proprio che è un titolo comprensivo di una risorsa che contiene più parti componenti intitolate distintamente."@it, "Titre propre qui est un titre global pour une ressource contenant plusieurs parties composantes titrées séparément."@fr, "Título inclusivo usado ya sea como el título propiamente dicho para un recurso que tiene contenido individual titulado separadamente, o como el título preferido para una compilación de dos o más obra."@es ;
    skos:inScheme <http://rdaregistry.info/termList/RDATerms> ;
    skos:narrower <http://rdaregistry.info/termList/RDATerms/1027> ;
    skos:prefLabel "collective title"@en, "titolo collettivo"@it, "titre collectif"@fr, "título colectivo"@es .

<http://rdaregistry.info/termList/RDATerms/1021>
    rdakit:toolkitDefinition "A discrete unit of intellectual content within a larger resource."@en ;
    rdakit:toolkitLabel "component part"@en ;
    reg:identifier <http://metadataregistry.org/concepts/8536> ;
    reg:status <http://metadataregistry.org/uri/RegStatus/1001> ;
    a skos:Concept ;
    skos:definition "A discrete unit of intellectual content within a larger resource."@en ;
    skos:inScheme <http://rdaregistry.info/termList/RDATerms> ;
    skos:prefLabel "component part"@en .

<http://rdaregistry.info/termList/RDATerms/1022>
    rdakit:toolkitDefinition "A description that combines one or more elements identifying a work and/or expression embodied in a manifestation with a description of the manifestation."@en, "Descripción que combina uno o más elementos que identifican una obra y/o expresión materializada en una manifestación con una descripción de una manifestación."@es, "Description qui combine un ou plusieurs éléments identifiant une œuvre et/ou une expression matérialisée dans une manifestation avec une description de la manifestation."@fr, "Descrizione che combina la descrizione di una manifestazione con uno o più elementi che identificano l'opera e/o l'espressione materializzate in quella manifestazione."@it ;
    rdakit:toolkitLabel "composite description"@en, "descripción compuesta"@es, "description composite"@fr, "descrizione composita"@it ;
    reg:identifier <http://metadataregistry.org/concepts/8537> ;
    reg:status <http://metadataregistry.org/uri/RegStatus/1001> ;
    a skos:Concept ;
    skos:definition "A description that combines one or more elements identifying a work and/or expression embodied in a manifestation with a description of the manifestation."@en, "Descripción que combina uno o más elementos que identifican una obra y/o expresión materializada en una manifestación con una descripción de una manifestación."@es, "Description qui combine un ou plusieurs éléments identifiant une œuvre et/ou une expression matérialisée dans une manifestation avec une description de la manifestation."@fr, "Descrizione che combina la descrizione di una manifestazione con uno o più elementi che identificano l'opera e/o l'espressione materializzate in quella manifestazione."@it ;
    skos:inScheme <http://rdaregistry.info/termList/RDATerms> ;
    skos:prefLabel "composite description"@en, "descripción compuesta"@es, "description composite"@fr, "descrizione composita"@it .

<http://rdaregistry.info/termList/RDATerms/1023>
    rdakit:toolkitDefinition "A surname consisting of two or more proper names, sometimes connected by a hyphen, or conjunction, and/or preposition."@en, "Cognome che consiste di due o più nomi propri, talvolta connessi da un trattino o una congiunzione e/o una preposizione."@it, "Nom de famille constitué de deux ou plusieurs noms propres parfois reliés par un trait d’union, une conjonction et/ou une préposition."@fr ;
    rdakit:toolkitLabel "cognome composto"@it, "compound surname"@en, "nom de famille composé"@fr ;
    reg:identifier <http://metadataregistry.org/concepts/8538> ;
    reg:status <http://metadataregistry.org/uri/RegStatus/1001> ;
    a skos:Concept ;
    skos:definition "A surname consisting of two or more proper names, sometimes connected by a hyphen, or conjunction, and/or preposition."@en, "Cognome che consiste di due o più nomi propri, talvolta connessi da un trattino o una congiunzione e/o una preposizione."@it, "Nom de famille constitué de deux ou plusieurs noms propres parfois reliés par un trait d’union, une conjonction et/ou une préposition."@fr ;
    skos:inScheme <http://rdaregistry.info/termList/RDATerms> ;
    skos:prefLabel "cognome composto"@it, "compound surname"@en, "nom de famille composé"@fr .

<http://rdaregistry.info/termList/RDATerms/1024>
    rdakit:toolkitDefinition "A description that describes the manifestation as a whole."@en, "Descripción en la que se describe al recurso como un todo."@es, "Description qui décrit la ressource dans son ensemble"@fr, "Descrizione che rappresenta la risorsa nel suo insieme"@it ;
    rdakit:toolkitLabel "comprehensive description"@en, "descripción integral"@es, "description globale"@fr, "descrizione comprensiva"@it ;
    reg:identifier <http://metadataregistry.org/concepts/8539> ;
    reg:status <http://metadataregistry.org/uri/RegStatus/1001> ;
    a skos:Concept ;
    skos:definition "A description that describes the manifestation as a whole."@en, "Descripción en la que se describe al recurso como un todo."@es, "Description qui décrit la ressource dans son ensemble"@fr, "Descrizione che rappresenta la risorsa nel suo insieme"@it ;
    skos:inScheme <http://rdaregistry.info/termList/RDATerms> ;
    skos:prefLabel "comprehensive description"@en, "descripción integral"@es, "description globale"@fr, "descrizione comprensiva"@it ;
    skos:scopeNote "A description for a map, a periodical, a collection of posters assembled by a library, or a kit consisting of a filmstrip, an audiotape, and a teacher’s manual, are included."@en .

<http://rdaregistry.info/termList/RDATerms/1025>
    rdakit:toolkitDefinition "A meeting of individuals or representatives of various bodies for the purpose of discussing and/or acting on topics of common interest or a meeting of representatives of a corporate body that constitutes its legislative or governing body."@en, "Incontro di persone o rappresentanti di vari enti per discutere e/o agire su temi di comune interesse o incontro dei rappresentanti di un ente che ne costituisce l'organo legislativo o di governo."@it ;
    rdakit:toolkitLabel "conference"@en, "conferenza"@it ;
    reg:identifier <http://metadataregistry.org/concepts/8540> ;
    reg:status <http://metadataregistry.org/uri/RegStatus/1001> ;
    a skos:Concept ;
    skos:definition "A meeting of individuals or representatives of various bodies for the purpose of discussing and/or acting on topics of common interest or a meeting of representatives of a corporate body that constitutes its legislative or governing body."@en, "Incontro di persone o rappresentanti di vari enti per discutere e/o agire su temi di comune interesse o incontro dei rappresentanti di un ente che ne costituisce l'organo legislativo o di governo."@it ;
    skos:inScheme <http://rdaregistry.info/termList/RDATerms> ;
    skos:prefLabel "conference"@en, "conferenza"@it .

<http://rdaregistry.info/termList/RDATerms/1026>
    rdakit:toolkitDefinition "A housing that is physically separable from the carrier being housed."@en, "Contenant qui est physiquement séparable de la ressource contenue."@fr, "Custodia della risorsa, che ne è fisicamente separabile."@it ;
    rdakit:toolkitLabel "container"@en, "conteneur"@fr, "contenitore"@it ;
    reg:identifier <http://metadataregistry.org/concepts/8541> ;
    reg:status <http://metadataregistry.org/uri/RegStatus/1001> ;
    a skos:Concept ;
    skos:definition "A housing that is physically separable from the carrier being housed."@en, "Contenant qui est physiquement séparable de la ressource contenue."@fr, "Custodia della risorsa, che ne è fisicamente separabile."@it ;
    skos:inScheme <http://rdaregistry.info/termList/RDATerms> ;
    skos:narrower <http://rdaregistry.info/termList/RDATerms/1054> ;
    skos:prefLabel "container"@en, "conteneur"@fr, "contenitore"@it ;
    skos:related <http://rdaregistry.info/termList/RDATerms/1016>, <http://rdaregistry.info/termList/RDATerms/1058>, <http://rdaregistry.info/termList/RDATerms/1086> ;
    skos:scopeNote "A container includes a box for a disc or videocassette, a sleeve for a videodisc, etc.; an insert visible through the housing is part of the container."@en .

<http://rdaregistry.info/termList/RDATerms/1027>
    rdakit:toolkitDefinition "A title used as a preferred title for a compilation containing two or more works by one agent, or two or more parts of a work."@en, "Titolo utilizzato come titolo preferito per una compilazione che contiene due o più opere di una persona, famiglia o ente, o due o più parti di un'opera."@it, "Titre utilisé comme titre privilégié pour une compilation contenant deux ou plusieurs œuvres d’une même personne, famille ou collectivité, ou deux ou plusieurs parties d’une œuvre."@fr ;
    rdakit:toolkitLabel "conventional collective title"@en, "titolo collettivo convenzionale"@it, "titre collectif conventionnel"@fr ;
    reg:identifier <http://metadataregistry.org/concepts/8542> ;
    reg:status <http://metadataregistry.org/uri/RegStatus/1001> ;
    a skos:Concept ;
    skos:broader <http://rdaregistry.info/termList/RDATerms/1020> ;
    skos:definition "A title used as a preferred title for a compilation containing two or more works by one agent, or two or more parts of a work."@en, "Titolo utilizzato come titolo preferito per una compilazione che contiene due o più opere di una persona, famiglia o ente, o due o più parti di un'opera."@it, "Titre utilisé comme titre privilégié pour une compilation contenant deux ou plusieurs œuvres d’une même personne, famille ou collectivité, ou deux ou plusieurs parties d’une œuvre."@fr ;
    skos:inScheme <http://rdaregistry.info/termList/RDATerms> ;
    skos:prefLabel "conventional collective title"@en, "titolo collettivo convenzionale"@it, "titre collectif conventionnel"@fr .

<http://rdaregistry.info/termList/RDATerms/1028>
    rdakit:toolkitDefinition "A name, other than the real or official name, by which a corporate body has come to be known."@en, "Nom, autre que le nom réel ou officiel, sous lequel une collectivité en est venue à être connue."@fr, "Nombre, diferente al nombre verdadero u oficial, mediante el cual llega a ser conocida una entidad corporativa, un lugar o un objeto."@es, "Nome, diverso dal nome reale o ufficiale, con cui un ente è conosciuto."@it ;
    rdakit:toolkitLabel "conventional name"@en, "nom conventionnel"@fr, "nombre convencional"@es, "nome convenzionale"@it ;
    reg:identifier <http://metadataregistry.org/concepts/8543> ;
    reg:status <http://metadataregistry.org/uri/RegStatus/1001> ;
    a skos:Concept ;
    skos:definition "A name, other than the real or official name, by which a corporate body has come to be known."@en, "Nom, autre que le nom réel ou officiel, sous lequel une collectivité en est venue à être connue."@fr, "Nombre, diferente al nombre verdadero u oficial, mediante el cual llega a ser conocida una entidad corporativa, un lugar o un objeto."@es, "Nome, diverso dal nome reale o ufficiale, con cui un ente è conosciuto."@it ;
    skos:inScheme <http://rdaregistry.info/termList/RDATerms> ;
    skos:prefLabel "conventional name"@en, "nom conventionnel"@fr, "nombre convencional"@es, "nome convenzionale"@it .

<http://rdaregistry.info/termList/RDATerms/1029>
    rdakit:toolkitDefinition "An indication that an RDA element, element sub-type, or sub-element is required to support specified user tasks according to the FRBR assessment of the value of each attribute and relationship."@en ;
    rdakit:toolkitLabel "core"@en ;
    reg:identifier <http://metadataregistry.org/concepts/8544> ;
    reg:status <http://metadataregistry.org/uri/RegStatus/1001> ;
    a skos:Concept ;
    skos:definition "An indication that an RDA element, element sub-type, or sub-element is required to support specified user tasks according to the FRBR assessment of the value of each attribute and relationship."@en ;
    skos:inScheme <http://rdaregistry.info/termList/RDATerms> ;
    skos:prefLabel "core"@en .

<http://rdaregistry.info/termList/RDATerms/1030>
    rdakit:toolkitDefinition "An outer protective material attached to a volume, consisting of both sides of the front and back panels and the spine to which they are joined."@en, "Envoltura protectora de un volumen, que consiste en de una hoja que cubre la parte frontal, el lomo del volumen y la parte posterior."@es, "Le matériau de protection externe fixé à un volume, constitué des deux faces des plats avant et arrière en plus du dos auquel ils sont liés."@fr, "Materiale protettivo esterno attaccato a un volume, che consiste di entrambi i lati delle coperture anteriore e posteriore e del dorso al quale esse sono unite."@it ;
    rdakit:toolkitLabel "copertina"@it, "couverture"@fr, "cover"@en, "cubierta"@es ;
    reg:identifier <http://metadataregistry.org/concepts/8545> ;
    reg:status <http://metadataregistry.org/uri/RegStatus/1001> ;
    a skos:Concept ;
    skos:definition "An outer protective material attached to a volume, consisting of both sides of the front and back panels and the spine to which they are joined."@en, "Envoltura protectora de un volumen, que consiste en de una hoja que cubre la parte frontal, el lomo del volumen y la parte posterior."@es, "Le matériau de protection externe fixé à un volume, constitué des deux faces des plats avant et arrière en plus du dos auquel ils sont liés."@fr, "Materiale protettivo esterno attaccato a un volume, che consiste di entrambi i lati delle coperture anteriore e posteriore e del dorso al quale esse sono unite."@it ;
    skos:inScheme <http://rdaregistry.info/termList/RDATerms> ;
    skos:prefLabel "copertina"@it, "couverture"@fr, "cover"@en, "cubierta"@es .

<http://rdaregistry.info/termList/RDATerms/1031>
    rdakit:toolkitDefinition "A collection of factual information presented in a structured form."@en, "Information factuelle présentée sous une forme structurée."@fr, "Informazione fattuale presentata in forma strutturata."@it ;
    rdakit:toolkitLabel "dataset"@en, "dataset"@it, "ensemble de données"@fr ;
    reg:identifier <http://metadataregistry.org/concepts/8546> ;
    reg:status <http://metadataregistry.org/uri/RegStatus/1001> ;
    a skos:Concept ;
    skos:definition "A collection of factual information presented in a structured form."@en, "Information factuelle présentée sous une forme structurée."@fr, "Informazione fattuale presentata in forma strutturata."@it ;
    skos:inScheme <http://rdaregistry.info/termList/RDATerms> ;
    skos:prefLabel "dataset"@en, "dataset"@it, "ensemble de données"@fr .

<http://rdaregistry.info/termList/RDATerms/1032>
    rdakit:toolkitDefinition "An earliest date a treaty or a protocol to a treaty was adopted by an international intergovernmental body or by an international conference, was opened for signing, was formally signed, was ratified, was proclaimed, etc."@en, "La date la plus ancienne où un traité ou un protocole d’un traité a été adopté par une organisation internationale intergouvernementale ou par une conférence internationale, a été ouvert à la signature, a été signé officiellement, a été ratifié, a été proclamé, etc."@fr, "La prima data in cui un trattato o il protocollo di un trattato è stato adottato da un ente intergovernativo internazionale o da una conferenza internazionale, è stato aperto alla firma, ratificato, proclamato, etc."@it ;
    rdakit:toolkitLabel "data di un trattato"@it, "date d’un traité"@fr, "date of a treaty"@en ;
    reg:identifier <http://metadataregistry.org/concepts/8547> ;
    reg:status <http://metadataregistry.org/uri/RegStatus/1001> ;
    a skos:Concept ;
    skos:definition "An earliest date a treaty or a protocol to a treaty was adopted by an international intergovernmental body or by an international conference, was opened for signing, was formally signed, was ratified, was proclaimed, etc."@en, "La date la plus ancienne où un traité ou un protocole d’un traité a été adopté par une organisation internationale intergouvernementale ou par une conférence internationale, a été ouvert à la signature, a été signé officiellement, a été ratifié, a été proclamé, etc."@fr, "La prima data in cui un trattato o il protocollo di un trattato è stato adottato da un ente intergovernativo internazionale o da una conferenza internazionale, è stato aperto alla firma, ratificato, proclamato, etc."@it ;
    skos:inScheme <http://rdaregistry.info/termList/RDATerms> ;
    skos:prefLabel "data di un trattato"@it, "date d’un traité"@fr, "date of a treaty"@en .

<http://rdaregistry.info/termList/RDATerms/1033>
    rdakit:toolkitDefinition "A year a law, etc., was promulgated or brought into force."@en, "Anno in cui una legge è stata promulgata o è entrata in vigore."@it, "L’année où une loi, etc. a été promulguée ou est entrée en vigueur."@fr ;
    rdakit:toolkitLabel "data di promulgazione di una legge"@it, "date de promulgation d’une loi, etc."@fr, "date of promulgation of a law, etc."@en ;
    reg:identifier <http://metadataregistry.org/concepts/8548> ;
    reg:status <http://metadataregistry.org/uri/RegStatus/1001> ;
    a skos:Concept ;
    skos:definition "A year a law, etc., was promulgated or brought into force."@en, "Anno in cui una legge è stata promulgata o è entrata in vigore."@it, "L’année où une loi, etc. a été promulguée ou est entrée en vigueur."@fr ;
    skos:inScheme <http://rdaregistry.info/termList/RDATerms> ;
    skos:prefLabel "data di promulgazione di una legge"@it, "date de promulgation d’une loi, etc."@fr, "date of promulgation of a law, etc."@en .

<http://rdaregistry.info/termList/RDATerms/1034>
    rdakit:toolkitDefinition "A word or phrase that describes an aspect of an entity."@en ;
    rdakit:toolkitLabel "designation"@en ;
    reg:identifier <http://metadataregistry.org/concepts/8549> ;
    reg:status <http://metadataregistry.org/uri/RegStatus/1001> ;
    a skos:Concept ;
    skos:definition "A word or phrase that describes an aspect of an entity."@en ;
    skos:inScheme <http://rdaregistry.info/termList/RDATerms> ;
    skos:prefLabel "designation"@en .

<http://rdaregistry.info/termList/RDATerms/1035>
    rdakit:toolkitDefinition "A set of data recording and identifying an entity."@en, "Conjunto de datos que registran e identifican a una entidad."@es, "Ensemble de données enregistrant et identifiant une entité."@fr, "Insieme di dati che registrano e identificano un'entità."@it ;
    rdakit:toolkitLabel "descripción"@es, "description"@en, "description"@fr, "descrizione"@it ;
    reg:identifier <http://metadataregistry.org/concepts/8550> ;
    reg:status <http://metadataregistry.org/uri/RegStatus/1001> ;
    a skos:Concept ;
    skos:definition "A set of data recording and identifying an entity."@en, "Conjunto de datos que registran e identifican a una entidad."@es, "Ensemble de données enregistrant et identifiant une entité."@fr, "Insieme di dati che registrano e identificano un'entità."@it ;
    skos:inScheme <http://rdaregistry.info/termList/RDATerms> ;
    skos:prefLabel "descripción"@es, "description"@en, "description"@fr, "descrizione"@it .

<http://rdaregistry.info/termList/RDATerms/1036>
    rdakit:toolkitDefinition "A title proper created by an agency preparing a description of a manifestation that bears no title itself and has no title associated with it that can be found in accompanying material, a published description of the manifestation, a reference source, etc."@en, "Titolo proprio creato da un'agenzia che redige una descrizione di una risorsa che non reca alcun titolo e non ha un titolo associato reperibile in altre fonti."@it, "Titre propre créé par une agence établissant la description d’une ressource qui ne porte par elle-même aucun titre et n’a pas de titre qu’il soit possible de trouver à lui associer dans d’autres sources"@fr ;
    rdakit:toolkitLabel "devised title"@en, "titolo escogitato"@it, "titre forgé"@fr ;
    reg:identifier <http://metadataregistry.org/concepts/8551> ;
    reg:status <http://metadataregistry.org/uri/RegStatus/1001> ;
    a skos:Concept ;
    skos:definition "A title proper created by an agency preparing a description of a manifestation that bears no title itself and has no title associated with it that can be found in accompanying material, a published description of the manifestation, a reference source, etc."@en, "Titolo proprio creato da un'agenzia che redige una descrizione di una risorsa che non reca alcun titolo e non ha un titolo associato reperibile in altre fonti."@it, "Titre propre créé par une agence établissant la description d’une ressource qui ne porte par elle-même aucun titre et n’a pas de titre qu’il soit possible de trouver à lui associer dans d’autres sources"@fr ;
    skos:inScheme <http://rdaregistry.info/termList/RDATerms> ;
    skos:prefLabel "devised title"@en, "titolo escogitato"@it, "titre forgé"@fr .

<http://rdaregistry.info/termList/RDATerms/1037>
    rdakit:toolkitDefinition "A resource, consisting of data and/or one or more programs, encoded for manipulation by a computerized device."@en, "Recurso (datos y/o programa(s)) codificado para su manipulación por un aparato computerizado."@es, "Ressource (données et/ou programme(s)) encodée en vue d’un traitement par un dispositif informatisé."@fr, "Risorsa (dati e/o programmi) codificata per la manipolazione mediante un dispositivo computerizzato."@it ;
    rdakit:toolkitLabel "digital resource"@en, "recurso digital"@es, "ressource numérique"@fr, "risorsa digitale"@it ;
    reg:identifier <http://metadataregistry.org/concepts/8552> ;
    reg:status <http://metadataregistry.org/uri/RegStatus/1001> ;
    a skos:Concept ;
    skos:definition "A resource, consisting of data and/or one or more programs, encoded for manipulation by a computerized device."@en, "Recurso (datos y/o programa(s)) codificado para su manipulación por un aparato computerizado."@es, "Ressource (données et/ou programme(s)) encodée en vue d’un traitement par un dispositif informatisé."@fr, "Risorsa (dati e/o programmi) codificata per la manipolazione mediante un dispositivo computerizzato."@it ;
    skos:inScheme <http://rdaregistry.info/termList/RDATerms> ;
    skos:prefLabel "digital resource"@en, "recurso digital"@es, "ressource numérique"@fr, "risorsa digitale"@it ;
    skos:scopeNote "El recurso puede requerir el uso de aparatos periféricos conectados directamente a un aparato computerizado (p.ej., una unidad de CD-ROM), un programa de aplicaciones (p.ej., un reproductor de un medio o un visualizador de imagen), y/o una conexión a una red de computadoras (p.ej., internet)."@es, "La ressource peut requérir l’utilisation d’un système périphérique directement connecté à un dispositif informatisé (par exemple, un lecteur de CD-ROM), un programme d’application (par exemple, un lecteur multimédia, un visionneur d’images) et/ou une connexion à un réseau d’ordinateurs (par exemple, Internet)."@fr, "La risorsa può richiedere una periferica direttamente connessa al dispositivo computerizzato (per esempio, un lettore CD-ROM), un'applicazione (per esempio, un programma di riproduzione, di visualizzazione di immagini) e/o la connessione a una rete di computer (per esempio, internet)."@it, "The resource may require the use of a peripheral device directly connected to a computerized device, an application program, and/or a connection to a computer network."@en .

<http://rdaregistry.info/termList/RDATerms/1038>
    rdakit:toolkitDefinition "A title of a musical work that is not just a form or musical genre, a tempo indication, a number of performers, or a type of liturgical text."@en, "Dans le contexte des œuvres musicales, titre qui n’est pas simplement une forme ou un genre musical, une indication de tempo, un nombre d’interprètes ou un type de texte liturgique."@fr, "En el contexto de las obras musicales, un título que no constituye solamente una forma o género musical, una indicación de tiempo, un número de interprétes o un tipo de texto litúrgico."@es, "Nel contesto delle opere musicali, titolo che non enuncia una forma o un genere musicale, un'indicazione di tempo, un numero di interpreti o un tipo di testo liturgico."@it ;
    rdakit:toolkitLabel "distinctive title"@en, "titolo distintivo"@it, "titre distinctif"@fr, "título distintivo"@es ;
    reg:identifier <http://metadataregistry.org/concepts/8553> ;
    reg:status <http://metadataregistry.org/uri/RegStatus/1001> ;
    a skos:Concept ;
    skos:definition "A title of a musical work that is not just a form or musical genre, a tempo indication, a number of performers, or a type of liturgical text."@en, "Dans le contexte des œuvres musicales, titre qui n’est pas simplement une forme ou un genre musical, une indication de tempo, un nombre d’interprètes ou un type de texte liturgique."@fr, "En el contexto de las obras musicales, un título que no constituye solamente una forma o género musical, una indicación de tiempo, un número de interprétes o un tipo de texto litúrgico."@es, "Nel contesto delle opere musicali, titolo che non enuncia una forma o un genere musicale, un'indicazione di tempo, un numero di interpreti o un tipo di testo liturgico."@it ;
    skos:inScheme <http://rdaregistry.info/termList/RDATerms> ;
    skos:prefLabel "distinctive title"@en, "titolo distintivo"@it, "titre distinctif"@fr, "título distintivo"@es .

<http://rdaregistry.info/termList/RDATerms/1039>
    rdakit:toolkitDefinition "A leaf of double size relative to the rest of a manifestation or item, folded in half at the fore-edge or top edge, with the fold uncut and no printing inside the fold, and typically bound at the inner margin."@en, "Feuillet de taille double, plié au niveau de la tranche latérale ou supérieure de la ressource."@fr, "Un foglio di dimensioni doppie che presenta una piega sul bordo anteriore o sul bordo superiore della risorsa."@it ;
    rdakit:toolkitLabel "double leaf"@en, "feuillet double"@fr, "foglio piegato"@it ;
    reg:identifier <http://metadataregistry.org/concepts/8554> ;
    reg:status <http://metadataregistry.org/uri/RegStatus/1001> ;
    a skos:Concept ;
    skos:definition "A leaf of double size relative to the rest of a manifestation or item, folded in half at the fore-edge or top edge, with the fold uncut and no printing inside the fold, and typically bound at the inner margin."@en, "Feuillet de taille double, plié au niveau de la tranche latérale ou supérieure de la ressource."@fr, "Un foglio di dimensioni doppie che presenta una piega sul bordo anteriore o sul bordo superiore della risorsa."@it ;
    skos:inScheme <http://rdaregistry.info/termList/RDATerms> ;
    skos:prefLabel "double leaf"@en, "feuillet double"@fr, "foglio piegato"@it .

<http://rdaregistry.info/termList/RDATerms/1040>
    rdakit:toolkitDefinition "A manifestation manufactured using a hand-press method, before the advent of machine printing in the nineteenth century."@en, "Materiali prodotti prima dell'introduzione della stampa meccanica, approssimativamente tra il 1825 e il 1830."@it ;
    rdakit:toolkitLabel "early printed resource"@en, "risorsa antiche a stampa"@it ;
    reg:identifier <http://metadataregistry.org/concepts/8555> ;
    reg:status <http://metadataregistry.org/uri/RegStatus/1001> ;
    a skos:Concept ;
    skos:definition "A manifestation manufactured using a hand-press method, before the advent of machine printing in the nineteenth century."@en, "Materiali prodotti prima dell'introduzione della stampa meccanica, approssimativamente tra il 1825 e il 1830."@it ;
    skos:inScheme <http://rdaregistry.info/termList/RDATerms> ;
    skos:prefLabel "A manifestation manufactured using a hand-press method, before the advent of machine printing in the nineteenth century."@en, "early printed resource"@en, "risorsa antiche a stampa"@it .

<http://rdaregistry.info/termList/RDATerms/1041>
    rdakit:toolkitDefinition "A word, character, or group of words and/or characters representing a distinct unit of bibliographic information."@en, "Mot, caractère ou groupe de mots et/ou de caractères représentant une unité distincte d’information bibliographique."@fr, "Parola, carattere o serie di parole e/o caratteri che rappresentano un'unità distinta d'informazione bibliografica."@it, "Sana, ilmaus tai sana - ja/tai merkkiryhmä, joka on bibliografisten tietojen erillinen yksikkö."@fi ;
    rdakit:toolkitLabel "element"@en, "elemento"@it, "elementti"@fi, "élément"@fr ;
    reg:identifier <http://metadataregistry.org/concepts/8556> ;
    reg:status <http://metadataregistry.org/uri/RegStatus/1001> ;
    a skos:Concept ;
    skos:definition "A word, character, or group of words and/or characters representing a distinct unit of bibliographic information."@en, "Mot, caractère ou groupe de mots et/ou de caractères représentant une unité distincte d’information bibliographique."@fr, "Parola, carattere o serie di parole e/o caratteri che rappresentano un'unità distinta d'informazione bibliografica."@it, "Sana, ilmaus tai sana - ja/tai merkkiryhmä, joka on bibliografisten tietojen erillinen yksikkö."@fi ;
    skos:inScheme <http://rdaregistry.info/termList/RDATerms> ;
    skos:prefLabel "element"@en, "elemento"@it, "elementti"@fi, "élément"@fr .

<http://rdaregistry.info/termList/RDATerms/1042>
    rdakit:toolkitDefinition "An elaborated see reference or see also reference that explains the circumstances under which the authorized access points involved should be consulted."@en, "Un rinviovedi o vedi anche redatto per spiegare i casi per i quali dovrebbero essere consultati i rispettivi punti d'accesso autorizzati."@it ;
    rdakit:toolkitLabel "explanatory reference"@en, "rinvio esplicativo"@it ;
    reg:identifier <http://metadataregistry.org/concepts/8557> ;
    reg:status <http://metadataregistry.org/uri/RegStatus/1001> ;
    a skos:Concept ;
    skos:definition "An elaborated see reference or see also reference that explains the circumstances under which the authorized access points involved should be consulted."@en, "Un rinviovedi o vedi anche redatto per spiegare i casi per i quali dovrebbero essere consultati i rispettivi punti d'accesso autorizzati."@it ;
    skos:inScheme <http://rdaregistry.info/termList/RDATerms> ;
    skos:prefLabel "explanatory reference"@en, "rinvio esplicativo"@it .

<http://rdaregistry.info/termList/RDATerms/1043>
    rdakit:toolkitDefinition "A descriptive tool providing access to a resource."@en, "Strumento descrittivo che fornisce accesso a una risorsa."@it ;
    rdakit:toolkitLabel "aiuto alla ricerca"@it, "finding aid"@en ;
    reg:identifier <http://metadataregistry.org/concepts/8558> ;
    reg:status <http://metadataregistry.org/uri/RegStatus/1001> ;
    a skos:Concept ;
    skos:definition "A descriptive tool providing access to a resource."@en, "Strumento descrittivo che fornisce accesso a una risorsa."@it ;
    skos:inScheme <http://rdaregistry.info/termList/RDATerms> ;
    skos:prefLabel "aiuto alla ricerca"@it, "finding aid"@en .

<http://rdaregistry.info/termList/RDATerms/1044>
    rdakit:toolkitDefinition "An element appearing in isolation, as opposed to appearing embedded in text, and in a prominent location."@en ;
    rdakit:toolkitLabel "formally presented"@en ;
    reg:identifier <http://metadataregistry.org/concepts/8559> ;
    reg:status <http://metadataregistry.org/uri/RegStatus/1001> ;
    a skos:Concept ;
    skos:definition "An element appearing in isolation, as opposed to appearing embedded in text, and in a prominent location."@en ;
    skos:inScheme <http://rdaregistry.info/termList/RDATerms> ;
    skos:prefLabel "formally presented"@en .

<http://rdaregistry.info/termList/RDATerms/1045>
    rdakit:toolkitDefinition "A pair or pairs of leaves that together form a distinctive unit for binding purposes."@en, "Uno o più coppie di carte – costituite da un foglio piegato, una parte di foglio piegata o numerosi fogli piegati inseriti l'uno nell'altro – che formano insieme un'unità distinta per la legatura."@it ;
    rdakit:toolkitLabel "fascicolo"@it, "gathering"@en ;
    reg:identifier <http://metadataregistry.org/concepts/8560> ;
    reg:status <http://metadataregistry.org/uri/RegStatus/1001> ;
    a skos:Concept ;
    skos:definition "A pair or pairs of leaves that together form a distinctive unit for binding purposes."@en, "Uno o più coppie di carte – costituite da un foglio piegato, una parte di foglio piegata o numerosi fogli piegati inseriti l'uno nell'altro – che formano insieme un'unità distinta per la legatura."@it ;
    skos:inScheme <http://rdaregistry.info/termList/RDATerms> ;
    skos:prefLabel "fascicolo"@it, "gathering"@en ;
    skos:scopeNote "A gathering may consist of a folded sheet, a fraction of a folded sheet, or several folded sheets tucked inside one another."@en .

<http://rdaregistry.info/termList/RDATerms/1046>
    rdakit:toolkitDefinition "A totality of executive, legislative, and judicial corporate bodies exercising the powers of a jurisdiction."@en, "Insieme degli organi (esecutivi, legislativi e giudiziari) che esercitano i poteri di una giurisdizione."@it, "L’ensemble des collectivités (exécutive, législative et judiciaire) exerçant les pouvoirs d’une juridiction."@fr ;
    rdakit:toolkitLabel "gouvernement"@fr, "government"@en, "governo"@it ;
    reg:identifier <http://metadataregistry.org/concepts/8561> ;
    reg:status <http://metadataregistry.org/uri/RegStatus/1001> ;
    a skos:Concept ;
    skos:definition "A totality of executive, legislative, and judicial corporate bodies exercising the powers of a jurisdiction."@en, "Insieme degli organi (esecutivi, legislativi e giudiziari) che esercitano i poteri di una giurisdizione."@it, "L’ensemble des collectivités (exécutive, législative et judiciaire) exerçant les pouvoirs d’une juridiction."@fr ;
    skos:inScheme <http://rdaregistry.info/termList/RDATerms> ;
    skos:prefLabel "gouvernement"@fr, "government"@en, "governo"@it .

<http://rdaregistry.info/termList/RDATerms/1047>
    rdakit:toolkitDefinition "An arrangement of passages of the Bible on the same topic into parallel columns so that similarities and differences may be compared readily, or an interweaving of such passages into a continuous text."@en ;
    rdakit:toolkitLabel "harmonie"@fr, "harmony"@en, "sinossi"@it ;
    reg:identifier <http://metadataregistry.org/concepts/8562> ;
    reg:status <http://metadataregistry.org/uri/RegStatus/1001> ;
    a skos:Concept ;
    skos:definition "An arrangement of passages of the Bible on the same topic into parallel columns so that similarities and differences may be compared readily, or an interweaving of such passages into a continuous text."@en ;
    skos:inScheme <http://rdaregistry.info/termList/RDATerms> ;
    skos:prefLabel "harmonie"@fr, "harmony"@en, "sinossi"@it .

<http://rdaregistry.info/termList/RDATerms/1048>
    rdakit:toolkitDefinition "A description that combines a comprehensive description of the whole manifestation with analytical descriptions of one or more of its parts."@en, "Descripción que combina una descripción integral del recurso completo con descripciones analíticas de una o más de sus partes."@es, "Description combinant une description globale de la ressource dans son ensemble et des descriptions analytiques d’une ou plusieurs de ses parties."@fr, "Descrizione che combina la descrizione comprensiva dell'intera risorsa con le descrizioni analitiche di una o più parti di essa."@it ;
    rdakit:toolkitLabel "descripción jerárquica"@es, "description hiérarchisée"@fr, "descrizione gerarchica"@it, "hierarchical description"@en ;
    reg:identifier <http://metadataregistry.org/concepts/8563> ;
    reg:status <http://metadataregistry.org/uri/RegStatus/1001> ;
    a skos:Concept ;
    skos:definition "A description that combines a comprehensive description of the whole manifestation with analytical descriptions of one or more of its parts."@en, "Descripción que combina una descripción integral del recurso completo con descripciones analíticas de una o más de sus partes."@es, "Description combinant une description globale de la ressource dans son ensemble et des descriptions analytiques d’une ou plusieurs de ses parties."@fr, "Descrizione che combina la descrizione comprensiva dell'intera risorsa con le descrizioni analitiche di una o più parti di essa."@it ;
    skos:inScheme <http://rdaregistry.info/termList/RDATerms> ;
    skos:prefLabel "descripción jerárquica"@es, "description hiérarchisée"@fr, "descrizione gerarchica"@it, "hierarchical description"@en .

<http://rdaregistry.info/termList/RDATerms/1049>
    rdakit:toolkitDefinition "A standard for subject access points and/or classification numbers used in determining the names or terms, other identifying attributes, and relationships representing what a work is about."@en, "Järjestelmä, jota kuvaileva yhteisö käyttää aiheeseen liittyvien hakutietojen ja/tai luokituskaavion luokkien merkitsemiseen."@fi ;
    rdakit:toolkitLabel "aihetta identifioiva käsitejärjestelmä"@fi, "identifiable subject system"@en ;
    reg:identifier <http://metadataregistry.org/concepts/8564> ;
    reg:status <http://metadataregistry.org/uri/RegStatus/1001> ;
    a skos:Concept ;
    skos:definition "A standard for subject access points and/or classification numbers used in determining the names or terms, other identifying attributes, and relationships representing what a work is about."@en, "Järjestelmä, jota kuvaileva yhteisö käyttää aiheeseen liittyvien hakutietojen ja/tai luokituskaavion luokkien merkitsemiseen."@fi ;
    skos:inScheme <http://rdaregistry.info/termList/RDATerms> ;
    skos:prefLabel "aihetta identifioiva käsitejärjestelmä"@fi, "identifiable subject system"@en ;
    skos:scopeNote "An identifiable subject system includes rules for application of terms, systematic combination of terminology such as pre- or post-coordination, and guidelines on cardinality and depth of assignment."@en, "Sitä voidaan käyttää määrittämään terminologiaa, muita identifioivia attribuutteja ja teoksen aihetta. Se voi myös sisältää termien soveltamista ja yhdistämistä koskevia ohjeita (esim. etuliite) ja suosituksia periaatteista ja tarkkuuden tasosta."@fi .

<http://rdaregistry.info/termList/RDATerms/1050>
    rdakit:toolkitDefinition "A descriptive audio or tactile language text that is attached to, or supplied with, a tactile image, map or diagram."@en, "Testo descrittivo audio o in linguaggio tattile allegato o fornito insieme a un'immagine, una carta geografica o un diagramma tattile."@it, "Texte descriptif audio ou tactile qui est joint à, ou fourni avec, une image, une carte ou un diagramme tactiles."@fr ;
    rdakit:toolkitLabel "description d’image"@fr, "descrizione dell'immagine"@it, "image description"@en ;
    reg:identifier <http://metadataregistry.org/concepts/8565> ;
    reg:status <http://metadataregistry.org/uri/RegStatus/1001> ;
    a skos:Concept ;
    skos:definition "A descriptive audio or tactile language text that is attached to, or supplied with, a tactile image, map or diagram."@en, "Testo descrittivo audio o in linguaggio tattile allegato o fornito insieme a un'immagine, una carta geografica o un diagramma tattile."@it, "Texte descriptif audio ou tactile qui est joint à, ou fourni avec, une image, une carte ou un diagramme tactiles."@fr ;
    skos:inScheme <http://rdaregistry.info/termList/RDATerms> ;
    skos:prefLabel "description d’image"@fr, "descrizione dell'immagine"@it, "image description"@en .

<http://rdaregistry.info/termList/RDATerms/1051>
    rdakit:toolkitDefinition "An international body created by intergovernmental action."@en, "Un ente internazionale creato per iniziativa intergovernativa."@it ;
    rdakit:toolkitLabel "ente intergovernativo internazionale"@it, "international intergovernmental body"@en ;
    reg:identifier <http://metadataregistry.org/concepts/8566> ;
    reg:status <http://metadataregistry.org/uri/RegStatus/1001> ;
    a skos:Concept ;
    skos:definition "An international body created by intergovernmental action."@en, "Un ente internazionale creato per iniziativa intergovernativa."@it ;
    skos:inScheme <http://rdaregistry.info/termList/RDATerms> ;
    skos:prefLabel "ente intergovernativo internazionale"@it, "international intergovernmental body"@en .

<http://rdaregistry.info/termList/RDATerms/1052>
    rdakit:toolkitDefinition "A successive part of a serial."@en ;
    rdakit:toolkitLabel "issue"@en ;
    reg:identifier <http://metadataregistry.org/concepts/8567> ;
    reg:status <http://metadataregistry.org/uri/RegStatus/1001> ;
    a skos:Concept ;
    skos:definition "A successive part of a serial."@en ;
    skos:inScheme <http://rdaregistry.info/termList/RDATerms> ;
    skos:prefLabel "issue"@en ;
    skos:related <http://rdaregistry.info/termList/RDATerms/1065> .

<http://rdaregistry.info/termList/RDATerms/1053>
    rdakit:toolkitDefinition "An instance of an integrating resource, either as first released or after it has been updated."@en, "Instance d’une ressource intégratrice, soit lors de sa première mise à disposition soit après une mise à jour."@fr, "Istanza di una risorsa integrativa, così come rilasciata la prima volta o dopo un aggiornamento."@it ;
    rdakit:toolkitLabel "iteration"@en, "iterazione"@it, "itération"@fr ;
    reg:identifier <http://metadataregistry.org/concepts/8568> ;
    reg:status <http://metadataregistry.org/uri/RegStatus/1001> ;
    a skos:Concept ;
    skos:definition "An instance of an integrating resource, either as first released or after it has been updated."@en, "Instance d’une ressource intégratrice, soit lors de sa première mise à disposition soit après une mise à jour."@fr, "Istanza di una risorsa integrativa, così come rilasciata la prima volta o dopo un aggiornamento."@it ;
    skos:inScheme <http://rdaregistry.info/termList/RDATerms> ;
    skos:prefLabel "iteration"@en, "iterazione"@it, "itération"@fr .

<http://rdaregistry.info/termList/RDATerms/1054>
    rdakit:toolkitDefinition "A detachable, protective wrapping of a volume, issued as part of a manifestation by a publisher, etc."@en, "La chemise de protection amovible d’un volume, distribuée comme faisant partie intégrante de la ressource par un éditeur, etc."@fr, "La copertura protettiva e staccabile di un volume, pubblicata come parte della risorsa da un editore."@it ;
    rdakit:toolkitLabel "jacket"@en, "jaquette"@fr, "sovraccoperta"@it ;
    reg:identifier <http://metadataregistry.org/concepts/8569> ;
    reg:status <http://metadataregistry.org/uri/RegStatus/1001> ;
    a skos:Concept ;
    skos:altLabel "book jacket"@en, "couvre-livre"@fr ;
    skos:broader <http://rdaregistry.info/termList/RDATerms/1026> ;
    skos:definition "A detachable, protective wrapping of a volume, issued as part of a manifestation by a publisher, etc."@en, "La chemise de protection amovible d’un volume, distribuée comme faisant partie intégrante de la ressource par un éditeur, etc."@fr, "La copertura protettiva e staccabile di un volume, pubblicata come parte della risorsa da un editore."@it ;
    skos:inScheme <http://rdaregistry.info/termList/RDATerms> ;
    skos:prefLabel "jacket"@en, "jaquette"@fr, "sovraccoperta"@it .

<http://rdaregistry.info/termList/RDATerms/1055>
    rdakit:toolkitDefinition "A constituent of an intangible manifestation."@en, "Componente de un recurso intangible, tal como un archivo digital."@es, "Componente di una risorsa intangibile."@it, "Partie constituante d’une ressource immatérielle telle qu’un fichier numérique."@fr ;
    rdakit:toolkitLabel "logical unit"@en, "unidad lógica"@es, "unità logica"@it, "unité logique"@fr ;
    reg:identifier <http://metadataregistry.org/concepts/8570> ;
    reg:status <http://metadataregistry.org/uri/RegStatus/1001> ;
    a skos:Concept ;
    skos:definition "A constituent of an intangible manifestation."@en, "Componente de un recurso intangible, tal como un archivo digital."@es, "Componente di una risorsa intangibile."@it, "Partie constituante d’une ressource immatérielle telle qu’un fichier numérique."@fr ;
    skos:inScheme <http://rdaregistry.info/termList/RDATerms> ;
    skos:prefLabel "logical unit"@en, "unidad lógica"@es, "unità logica"@it, "unité logique"@fr ;
    skos:scopeNote "A digital file is included."@en .

<http://rdaregistry.info/termList/RDATerms/1056>
    rdakit:toolkitDefinition "A series that contains one or more subseries."@en, "Serie che contiene una o più sottoserie."@it, "Una serie que contiene una o más subseries."@es ;
    rdakit:toolkitLabel "main series"@en, "serie principal"@es, "serie principale"@it ;
    reg:identifier <http://metadataregistry.org/concepts/8571> ;
    reg:status <http://metadataregistry.org/uri/RegStatus/1001> ;
    a skos:Concept ;
    skos:definition "A series that contains one or more subseries."@en, "Serie che contiene una o più sottoserie."@it, "Una serie que contiene una o más subseries."@es ;
    skos:inScheme <http://rdaregistry.info/termList/RDATerms> ;
    skos:prefLabel "main series"@en, "serie principal"@es, "serie principale"@it .

<http://rdaregistry.info/termList/RDATerms/1057>
    rdakit:toolkitDefinition "A number of related but physically separate and bibliographically distinct cartographic units intended to form a single group, collectively identified by any commonly occurring unifying characteristic or combination of characteristics."@en, "Numero di unità cartografiche correlate ma fisicamente separate e bibliograficamente distinte, destinate a formare un gruppo unico."@it, "Plusieurs unités bibliographiques cartographiques distinctes et physiquement séparées mais qui sont associées et prévues pour former un ensemble unique."@fr, "Un número de unidades cartográficas relacionadas pero físicamente separadas y bibliográficamente distintas, pensadas para formar un solo grupo individual."@es ;
    rdakit:toolkitLabel "map series"@en, "serie cartográfica"@es, "serie di carte geografiche"@it, "série cartographique"@fr ;
    reg:identifier <http://metadataregistry.org/concepts/8572> ;
    reg:status <http://metadataregistry.org/uri/RegStatus/1001> ;
    a skos:Concept ;
    skos:definition "A number of related but physically separate and bibliographically distinct cartographic units intended to form a single group, collectively identified by any commonly occurring unifying characteristic or combination of characteristics."@en, "Numero di unità cartografiche correlate ma fisicamente separate e bibliograficamente distinte, destinate a formare un gruppo unico."@it, "Plusieurs unités bibliographiques cartographiques distinctes et physiquement séparées mais qui sont associées et prévues pour former un ensemble unique."@fr, "Un número de unidades cartográficas relacionadas pero físicamente separadas y bibliográficamente distintas, pensadas para formar un solo grupo individual."@es ;
    skos:inScheme <http://rdaregistry.info/termList/RDATerms> ;
    skos:prefLabel "map series"@en, "serie cartográfica"@es, "serie di carte geografiche"@it, "série cartographique"@fr ;
    skos:scopeNote "En su tratamiento bibliográfico, el grupo se identifica colectivamente mediante una característica común unificadora o a través de una combinación de características, incluyendo una designación común (p.ej., un título colectivo, un número o una combinación de ambos); un sistema de identificación de hojas (incluyendo los sistemas de numeración sucesiva o cronológica); la escala; el editor; especificaciones cartográficas; formato uniforme; etc."@es .

<http://rdaregistry.info/termList/RDATerms/1058>
    rdakit:toolkitDefinition "A means used to convey information or artistic content."@en, "Le moyen utilisé pour communiquer un contenu informatif ou artistique."@fr, "Los medios utilizados para transmitir información o contenido artístico."@es, "Mezzi utilizzati per trasmettere le informazioni o il contenuto artistico."@it ;
    rdakit:toolkitLabel "media"@en, "media"@it, "medios"@es, "média"@fr ;
    reg:identifier <http://metadataregistry.org/concepts/8573> ;
    reg:status <http://metadataregistry.org/uri/RegStatus/1001> ;
    a skos:Concept ;
    skos:definition "A means used to convey information or artistic content."@en, "Le moyen utilisé pour communiquer un contenu informatif ou artistique."@fr, "Los medios utilizados para transmitir información o contenido artístico."@es, "Mezzi utilizzati per trasmettere le informazioni o il contenuto artistico."@it ;
    skos:inScheme <http://rdaregistry.info/termList/RDATerms> ;
    skos:prefLabel "media"@en, "media"@it, "medios"@es, "média"@fr ;
    skos:related <http://rdaregistry.info/termList/RDATerms/1016>, <http://rdaregistry.info/termList/RDATerms/1026>, <http://rdaregistry.info/termList/RDATerms/1086> .

<http://rdaregistry.info/termList/RDATerms/1059>
    rdakit:toolkitDefinition "A film bearing a number of microimages in linear array."@en, "Film portant une série de micro-images disposées de façon linéaire."@fr, "Película que contiene un número de microimágenes en forma lineal."@es ;
    rdakit:toolkitLabel "microfilm"@en, "microfilm"@fr, "microfilme"@es ;
    reg:identifier <http://metadataregistry.org/concepts/8574> ;
    reg:status <http://metadataregistry.org/uri/RegStatus/1001> ;
    a skos:Concept ;
    skos:definition "A film bearing a number of microimages in linear array."@en, "Film portant une série de micro-images disposées de façon linéaire."@fr, "Película que contiene un número de microimágenes en forma lineal."@es ;
    skos:inScheme <http://rdaregistry.info/termList/RDATerms> ;
    skos:prefLabel "microfilm"@en, "microfilm"@fr, "microfilme"@es .

<http://rdaregistry.info/termList/RDATerms/1060>
    rdakit:toolkitDefinition "A resource that is complete in one part or intended to be completed within a finite number of parts."@en, "Recurso que está completo en una parte o que se tiene el propósito de completar con un número finito de partes."@es, "Ressource complète en une seule partie ou destinée à être complète en un nombre déterminé de parties."@fr, "Risorsa completa in una sola parte o destinata a essere completata in un numero finito di parti."@it ;
    rdakit:toolkitLabel "monografia"@it, "monografía"@es, "monograph"@en, "monographie"@fr ;
    reg:identifier <http://metadataregistry.org/concepts/8575> ;
    reg:status <http://metadataregistry.org/uri/RegStatus/1001> ;
    a skos:Concept ;
    skos:definition "A resource that is complete in one part or intended to be completed within a finite number of parts."@en, "Recurso que está completo en una parte o que se tiene el propósito de completar con un número finito de partes."@es, "Ressource complète en une seule partie ou destinée à être complète en un nombre déterminé de parties."@fr, "Risorsa completa in una sola parte o destinata a essere completata in un numero finito di parti."@it ;
    skos:inScheme <http://rdaregistry.info/termList/RDATerms> ;
    skos:prefLabel "monografia"@it, "monografía"@es, "monograph"@en, "monographie"@fr .

<http://rdaregistry.info/termList/RDATerms/1061>
    rdakit:toolkitDefinition "A form of presentation, in an ISBD display, of descriptive data based on the division of information into two or more levels."@en, "Dans un affichage ISBD, une description à plusieurs niveaux est une forme de présentation des données descriptives basée sur la répartition de l’information sur deux ou plusieurs niveaux."@fr, "En una muestra de ISBD, una descripción multinivel es una forma de presentación de datos descriptivos basados en la división de información descriptiva en dos o más niveles."@es, "In una visualizzazione ISBD, la descrizione a più livelli è una forma di presentazione dei dati descrittivi basata sulla suddivisione delle informazioni descrittive su due o più livelli."@it ;
    rdakit:toolkitLabel "descripción multinivel"@es, "description à plusieurs niveaux"@fr, "descrizione a più livelli"@it, "multilevel description"@en ;
    reg:identifier <http://metadataregistry.org/concepts/8576> ;
    reg:status <http://metadataregistry.org/uri/RegStatus/1001> ;
    a skos:Concept ;
    skos:definition "A form of presentation, in an ISBD display, of descriptive data based on the division of information into two or more levels."@en, "Dans un affichage ISBD, une description à plusieurs niveaux est une forme de présentation des données descriptives basée sur la répartition de l’information sur deux ou plusieurs niveaux."@fr, "En una muestra de ISBD, una descripción multinivel es una forma de presentación de datos descriptivos basados en la división de información descriptiva en dos o más niveles."@es, "In una visualizzazione ISBD, la descrizione a più livelli è una forma di presentazione dei dati descrittivi basata sulla suddivisione delle informazioni descrittive su due o più livelli."@it ;
    skos:inScheme <http://rdaregistry.info/termList/RDATerms> ;
    skos:prefLabel "descripción multinivel"@es, "description à plusieurs niveaux"@fr, "descrizione a più livelli"@it, "multilevel description"@en ;
    skos:scopeNote "El primer nivel contiene información común al total o recurso principal. El segundo y niveles subsecuentes contienen información sobre la parte individual."@es, "Il primo livello contiene informazioni comuni a tutta la risorsa o a quella principale. Il secondo livello e quelli successivi contengono informazioni sulle parti singole."@it, "Le premier niveau contient l’information commune à l’ensemble de la ressource ou à la ressource principale. Le deuxième niveau et les niveaux suivants contiennent l’information sur la partie individuelle."@fr, "The first level contains information common to the whole or main resource. The second and subsequent levels contain information about an individual part."@en .

<http://rdaregistry.info/termList/RDATerms/1062>
    rdakit:toolkitDefinition "A word, character, or group of words and/or characters by which an entity is known."@en, "Mot, caractère ou groupe de mots et/ou de caractères sous lequel une personne, famille ou collectivité est connue."@fr, "Palabra, carácter o grupo de palabras y/o caracteres mediante el cual se conoce una entidad."@es, "Parola, carattere o serie di parole e/o caratteri con cui una persona, famiglia o ente è conosciuto."@it ;
    rdakit:toolkitLabel "name"@en, "nom"@fr, "nombre"@es, "nome"@it ;
    reg:identifier <http://metadataregistry.org/concepts/8577> ;
    reg:status <http://metadataregistry.org/uri/RegStatus/1001> ;
    a skos:Concept ;
    skos:definition "A word, character, or group of words and/or characters by which an entity is known."@en, "Mot, caractère ou groupe de mots et/ou de caractères sous lequel une personne, famille ou collectivité est connue."@fr, "Palabra, carácter o grupo de palabras y/o caracteres mediante el cual se conoce una entidad."@es, "Parola, carattere o serie di parole e/o caratteri con cui una persona, famiglia o ente è conosciuto."@it ;
    skos:inScheme <http://rdaregistry.info/termList/RDATerms> ;
    skos:prefLabel "name"@en, "nom"@fr, "nombre"@es, "nome"@it .

<http://rdaregistry.info/termList/RDATerms/1063>
    rdakit:toolkitDefinition "A line marking the outer edge of a map or chart, separating its detail from any border or margin."@en ;
    rdakit:toolkitLabel "neat line"@en ;
    reg:identifier <http://metadataregistry.org/concepts/8578> ;
    reg:status <http://metadataregistry.org/uri/RegStatus/1001> ;
    a skos:Concept ;
    skos:definition "A line marking the outer edge of a map or chart, separating its detail from any border or margin."@en ;
    skos:inScheme <http://rdaregistry.info/termList/RDATerms> ;
    skos:prefLabel "neat line"@en .

<http://rdaregistry.info/termList/RDATerms/1064>
    rdakit:toolkitDefinition "A manifestation that does not contain identifying information."@en ;
    rdakit:toolkitLabel "non-self-describing manifestation"@en ;
    reg:identifier <http://metadataregistry.org/concepts/8579> ;
    reg:status <http://metadataregistry.org/uri/RegStatus/1001> ;
    a skos:Concept ;
    skos:definition "A manifestation that does not contain identifying information."@en ;
    skos:inScheme <http://rdaregistry.info/termList/RDATerms> ;
    skos:prefLabel "non-self-describing manifestation"@en .

<http://rdaregistry.info/termList/RDATerms/1065>
    rdakit:toolkitDefinition "A unit into which a resource has been permanently divided by a publisher, manufacturer, etc."@en ;
    rdakit:toolkitLabel "part"@en, "parte"@it ;
    reg:identifier <http://metadataregistry.org/concepts/8580> ;
    reg:status <http://metadataregistry.org/uri/RegStatus/1001> ;
    a skos:Concept ;
    skos:definition "A unit into which a resource has been permanently divided by a publisher, manufacturer, etc."@en ;
    skos:inScheme <http://rdaregistry.info/termList/RDATerms> ;
    skos:prefLabel "part"@en, "parte"@it ;
    skos:related <http://rdaregistry.info/termList/RDATerms/1052> .

<http://rdaregistry.info/termList/RDATerms/1066>
    rdakit:toolkitDefinition "A name derived from the given name of a father."@en, "Nom formé à partir du prénom du père."@fr, "Nombre derivado del nombre de pila de un padre."@es, "Nome derivato dal nome proprio del padre."@it ;
    rdakit:toolkitLabel "patronimico"@it, "patronyme"@fr, "patronymic"@en, "patronímico"@es ;
    reg:identifier <http://metadataregistry.org/concepts/8581> ;
    reg:status <http://metadataregistry.org/uri/RegStatus/1001> ;
    a skos:Concept ;
    skos:definition "A name derived from the given name of a father."@en, "Nom formé à partir du prénom du père."@fr, "Nombre derivado del nombre de pila de un padre."@es, "Nome derivato dal nome proprio del padre."@it ;
    skos:inScheme <http://rdaregistry.info/termList/RDATerms> ;
    skos:prefLabel "patronimico"@it, "patronyme"@fr, "patronymic"@en, "patronímico"@es .

<http://rdaregistry.info/termList/RDATerms/1067>
    rdakit:toolkitDefinition "A constituent of a tangible manifestation."@en, "Componente di una risorsa tangibile."@it, "Composant d’une ressource matérielle, tel qu’un volume, une cassette audio ou une bobine de film."@fr ;
    rdakit:toolkitLabel "physical unit"@en, "unità fisica"@it, "unité physique"@fr ;
    reg:identifier <http://metadataregistry.org/concepts/8582> ;
    reg:status <http://metadataregistry.org/uri/RegStatus/1001> ;
    a skos:Concept ;
    skos:definition "A constituent of a tangible manifestation."@en, "Componente di una risorsa tangibile."@it, "Composant d’une ressource matérielle, tel qu’un volume, une cassette audio ou une bobine de film."@fr ;
    skos:inScheme <http://rdaregistry.info/termList/RDATerms> ;
    skos:prefLabel "physical unit"@en, "unità fisica"@it, "unité physique"@fr ;
    skos:scopeNote "A physical unit includes a volume, audiocassette, or film reel."@en .

<http://rdaregistry.info/termList/RDATerms/1068>
    rdakit:toolkitDefinition "A leaf, usually containing illustrative content, that does not form part of either the preliminary or the main sequence of pages or leaves."@en, "Carta che presenta contenuto illustrativo, corredato o meno da testo esplicativo, che non fa parte delle parti preliminari né della sequenza principale delle pagine o carte."@it ;
    rdakit:toolkitLabel "plate"@en, "tavola"@it ;
    reg:identifier <http://metadataregistry.org/concepts/8583> ;
    reg:status <http://metadataregistry.org/uri/RegStatus/1001> ;
    a skos:Concept ;
    skos:definition "A leaf, usually containing illustrative content, that does not form part of either the preliminary or the main sequence of pages or leaves."@en, "Carta che presenta contenuto illustrativo, corredato o meno da testo esplicativo, che non fa parte delle parti preliminari né della sequenza principale delle pagine o carte."@it ;
    skos:inScheme <http://rdaregistry.info/termList/RDATerms> ;
    skos:prefLabel "plate"@en, "tavola"@it .

<http://rdaregistry.info/termList/RDATerms/1069>
    rdakit:toolkitDefinition "A name or form of name chosen as the basis for an authorized access point representing an entity."@en, "El nombre o la forma del nombre elegida como base para el punto de acceso autorizado que representa una entidad."@es, "Le nom ou la forme de nom choisie pour servir d’élément de base du point d’accès autorisé représentant une entité."@fr, "Nimi tai nimen muoto, joka on valittu henkilön, suvun tai yhteisön tunnistamiseksi."@fi, "Nome o forma del nome scelti come base per il punto d'accesso autorizzato che rappresenta un'entità."@it ;
    rdakit:toolkitLabel "ensisijainen nimi"@fi, "nom privilégié"@fr, "nombre preferido"@es, "nome preferito"@it, "preferred name"@en ;
    reg:identifier <http://metadataregistry.org/concepts/8584> ;
    reg:status <http://metadataregistry.org/uri/RegStatus/1001> ;
    a skos:Concept ;
    skos:definition "A name or form of name chosen as the basis for an authorized access point representing an entity."@en, "El nombre o la forma del nombre elegida como base para el punto de acceso autorizado que representa una entidad."@es, "Le nom ou la forme de nom choisie pour servir d’élément de base du point d’accès autorisé représentant une entité."@fr, "Nimi tai nimen muoto, joka on valittu henkilön, suvun tai yhteisön tunnistamiseksi."@fi, "Nome o forma del nome scelti come base per il punto d'accesso autorizzato che rappresenta un'entità."@it ;
    skos:inScheme <http://rdaregistry.info/termList/RDATerms> ;
    skos:prefLabel "ensisijainen nimi"@fi, "nom privilégié"@fr, "nombre preferido"@es, "nome preferito"@it, "preferred name"@en .

<http://rdaregistry.info/termList/RDATerms/1070>
    rdakit:toolkitDefinition "A relationship between a work, expression, manifestation, or item that is inherent in the FRBR definitions of those entities."@en ;
    rdakit:toolkitLabel "primary relationship"@en ;
    reg:identifier <http://metadataregistry.org/concepts/8585> ;
    reg:status <http://metadataregistry.org/uri/RegStatus/1001> ;
    a skos:Concept ;
    skos:definition "A relationship between a work, expression, manifestation, or item that is inherent in the FRBR definitions of those entities."@en ;
    skos:inScheme <http://rdaregistry.info/termList/RDATerms> ;
    skos:prefLabel "primary relationship"@en .

<http://rdaregistry.info/termList/RDATerms/1071>
    rdakit:toolkitDefinition "A treaty amending and supplementing another treaty."@en, "Traité amendant et complétant un autre traité."@fr, "Trattato che modifica e integra un altro trattato."@it ;
    rdakit:toolkitLabel "protocol"@en, "protocole"@fr, "protocollo"@it ;
    reg:identifier <http://metadataregistry.org/concepts/8586> ;
    reg:status <http://metadataregistry.org/uri/RegStatus/1001> ;
    a skos:Concept ;
    skos:definition "A treaty amending and supplementing another treaty."@en, "Traité amendant et complétant un autre traité."@fr, "Trattato che modifica e integra un altro trattato."@it ;
    skos:inScheme <http://rdaregistry.info/termList/RDATerms> ;
    skos:prefLabel "protocol"@en, "protocole"@fr, "protocollo"@it .

<http://rdaregistry.info/termList/RDATerms/1072>
    rdakit:toolkitDefinition "A name used by a person, either alone or in collaboration with others, that is not the person’s real name."@en, "Nom utilisé par une personne (seule ou en collaboration avec d’autres personnes) et qui n’est pas son nom véritable."@fr, "Nome utilizzato da una persona (da sola o in collaborazione con altri), diverso dal nome reale."@it, "Un nombre utilizado por una persona (ya sea por sí sola o en colaboración con otros), que no es el nombre real de la persona."@es ;
    rdakit:toolkitLabel "pseudonimo"@it, "pseudonym"@en, "pseudonyme"@fr, "seudónimo"@es ;
    reg:identifier <http://metadataregistry.org/concepts/8587> ;
    reg:status <http://metadataregistry.org/uri/RegStatus/1001> ;
    a skos:Concept ;
    skos:definition "A name used by a person, either alone or in collaboration with others, that is not the person’s real name."@en, "Nom utilisé par une personne (seule ou en collaboration avec d’autres personnes) et qui n’est pas son nom véritable."@fr, "Nome utilizzato da una persona (da sola o in collaborazione con altri), diverso dal nome reale."@it, "Un nombre utilizado por una persona (ya sea por sí sola o en colaboración con otros), que no es el nombre real de la persona."@es ;
    skos:inScheme <http://rdaregistry.info/termList/RDATerms> ;
    skos:prefLabel "pseudonimo"@it, "pseudonym"@en, "pseudonyme"@fr, "seudónimo"@es .

<http://rdaregistry.info/termList/RDATerms/1073>
    rdakit:toolkitDefinition "A direction from one access point to another."@en, "Rimando da un punto d'accesso a un altro."@it ;
    rdakit:toolkitLabel "reference"@en, "rinvio"@it ;
    reg:identifier <http://metadataregistry.org/concepts/8588> ;
    reg:status <http://metadataregistry.org/uri/RegStatus/1001> ;
    a skos:Concept ;
    skos:definition "A direction from one access point to another."@en, "Rimando da un punto d'accesso a un altro."@it ;
    skos:inScheme <http://rdaregistry.info/termList/RDATerms> ;
    skos:prefLabel "reference"@en, "rinvio"@it .

<http://rdaregistry.info/termList/RDATerms/1074>
    rdakit:toolkitDefinition "A source from which authoritative information may be obtained."@en, "Qualsiasi fonte da cui si possano ottenere informazioni autorevoli, compresi gli archivi di autorità, opere di consultazione, etc."@it, "Toda fuente de la cual se ha obtenido información autorizada."@es, "Toute source d’information faisant autorité, y compris les fichiers d’autorité, les ouvrages de référence, etc."@fr ;
    rdakit:toolkitLabel "fonte di reference"@it, "fuente de referencia"@es, "reference source"@en, "source de référence"@fr ;
    reg:identifier <http://metadataregistry.org/concepts/8589> ;
    reg:status <http://metadataregistry.org/uri/RegStatus/1001> ;
    a skos:Concept ;
    skos:definition "A source from which authoritative information may be obtained."@en, "Qualsiasi fonte da cui si possano ottenere informazioni autorevoli, compresi gli archivi di autorità, opere di consultazione, etc."@it, "Toda fuente de la cual se ha obtenido información autorizada."@es, "Toute source d’information faisant autorité, y compris les fichiers d’autorité, les ouvrages de référence, etc."@fr ;
    skos:inScheme <http://rdaregistry.info/termList/RDATerms> ;
    skos:prefLabel "fonte di reference"@it, "fuente de referencia"@es, "reference source"@en, "source de référence"@fr ;
    skos:scopeNote "A reference source includes an authority file, a reference work, etc."@en, "Incluye archivos de autoridad, fuentes de referencia, etc."@es .

<http://rdaregistry.info/termList/RDATerms/1075>
    rdakit:toolkitDefinition "A designator that indicates the nature of a relationship between entities represented by authorized access points, descriptions, and/or identifiers."@en, "Designador que indica la naturaleza de la relación entre las entidades representadas mediante puntos de acceso autorizados, descriptores y/o identificadores."@es, "Designatore che indica la natura della relazione tra entità rappresentate da un punto d'accesso autorizzato, descrizioni e/o identificatori."@it, "Indicateur qui définit la nature de la relation entre des entités représentées par des points d’accès autorisés, des descriptions et/ou des identifiants."@fr ;
    rdakit:toolkitLabel "designador de relación"@es, "designatore di relazione"@it, "indicateur de relation"@fr, "relationship designator"@en ;
    reg:identifier <http://metadataregistry.org/concepts/8590> ;
    reg:status <http://metadataregistry.org/uri/RegStatus/1001> ;
    a skos:Concept ;
    skos:definition "A designator that indicates the nature of a relationship between entities represented by authorized access points, descriptions, and/or identifiers."@en, "Designador que indica la naturaleza de la relación entre las entidades representadas mediante puntos de acceso autorizados, descriptores y/o identificadores."@es, "Designatore che indica la natura della relazione tra entità rappresentate da un punto d'accesso autorizzato, descrizioni e/o identificatori."@it, "Indicateur qui définit la nature de la relation entre des entités représentées par des points d’accès autorisés, des descriptions et/ou des identifiants."@fr ;
    skos:inScheme <http://rdaregistry.info/termList/RDATerms> ;
    skos:prefLabel "designador de relación"@es, "designatore di relazione"@it, "indicateur de relation"@fr, "relationship designator"@en .

<http://rdaregistry.info/termList/RDATerms/1076>
    rdakit:toolkitDefinition "An exact copy of the content of a manifestation or item made by mechanical or electronic means."@en, "Copia esatta del contenuto di una risorsa ottenuta mediante mezzi meccanici o elettronici."@it, "Copia exacta del contenido de un recurso, creada mediante medios mecánicos o electrónicos."@es ;
    rdakit:toolkitLabel "reproducción"@es, "reproduction"@en, "reproduction"@fr, "riproduzione"@it ;
    reg:identifier <http://metadataregistry.org/concepts/8591> ;
    reg:status <http://metadataregistry.org/uri/RegStatus/1001> ;
    a skos:Concept ;
    skos:definition "An exact copy of the content of a manifestation or item made by mechanical or electronic means."@en, "Copia esatta del contenuto di una risorsa ottenuta mediante mezzi meccanici o elettronici."@it, "Copia exacta del contenido de un recurso, creada mediante medios mecánicos o electrónicos."@es, "Copie exacte du contenu d’une ressource faite par un moyen mécanique ou électronique."@fr ;
    skos:inScheme <http://rdaregistry.info/termList/RDATerms> ;
    skos:prefLabel "reproducción"@es, "reproduction"@en, "reproduction"@fr, "riproduzione"@it .

<http://rdaregistry.info/termList/RDATerms/1077>
    rdakit:toolkitDefinition "A work, expression, manifestation or item."@en, "Obra, expresión, manifestación o ítem."@es, "Opera, espressione, manifestazione o item."@it, "Œuvre, expression, manifestation ou item."@fr ;
    rdakit:toolkitLabel "recurso"@es, "resource"@en, "ressource"@fr, "risorsa"@it ;
    reg:identifier <http://metadataregistry.org/concepts/8592> ;
    reg:status <http://metadataregistry.org/uri/RegStatus/1001> ;
    a skos:Concept ;
    skos:definition "A work, expression, manifestation or item."@en, "Obra, expresión, manifestación o ítem."@es, "Opera, espressione, manifestazione o item."@it, "Œuvre, expression, manifestation ou item."@fr ;
    skos:inScheme <http://rdaregistry.info/termList/RDATerms> ;
    skos:prefLabel "recurso"@es, "resource"@en, "ressource"@fr, "risorsa"@it ;
    skos:scopeNote "A resource can be an individual entity, an aggregate, or a component of such an entity.  It can be a tangible or intangible entity."@en, "El término incluye no solamente a una entidad individual sino también a los agregados y los componentes de dichas entidades (p.ej., mapas de tres hojas; una diapositiva individual que forma parte de un conjunto de veinte; o un artículo de una entrega de una revista especializada). Puede referirse a una entidad tangible (p.ej., un audiocasete) o a una entidad intangible (p.ej., un sitio Web)"@es, "Il termine include non solo un'entità individuale ma anche aggregati e componenti di tali entità (per esempio, tre fogli di carte geografiche, una diapositiva singola pubblicata come parte di un insieme di venti diapositive, l'articolo di un fascicolo di un giornale accademico). Può indicare un'entità tangibile (per esempio, un'audiocassetta) o un'entità intangibile (per esempio, un sito web)."@it, "Le terme inclut non seulement les entités individuelles mais aussi les agrégats et les composantes de ces entités (par exemple, trois cartes en feuilles, une diapositive isolée publiée comme partie d’un lot de vingt, un article dans une livraison d’une revue savante). Il peut désigner une entité matérielle (par exemple, une cassette audio) ou une entité immatérielle (par exemple, un site Web)."@fr .

<http://rdaregistry.info/termList/RDATerms/1078>
    rdakit:toolkitDefinition "A title, or abbreviated title, that is repeated at the head or foot of each page or leaf."@en, "Titre, ou titre abrégé, répété en tête ou en pied de chaque page ou feuillet."@fr ;
    rdakit:toolkitLabel "running title"@en, "titre courant"@fr ;
    reg:identifier <http://metadataregistry.org/concepts/8593> ;
    reg:status <http://metadataregistry.org/uri/RegStatus/1001> ;
    a skos:Concept ;
    skos:definition "A title, or abbreviated title, that is repeated at the head or foot of each page or leaf."@en, "Titre, ou titre abrégé, répété en tête ou en pied de chaque page ou feuillet."@fr ;
    skos:inScheme <http://rdaregistry.info/termList/RDATerms> ;
    skos:prefLabel "running title"@en, "titre courant"@fr .

<http://rdaregistry.info/termList/RDATerms/1079>
    rdakit:toolkitDefinition "A single or composite sheet containing text and/or images, originally produced rolled, and intended to be unrolled a portion at a time for reading or viewing."@en ;
    rdakit:toolkitLabel "scroll"@en ;
    reg:identifier <http://metadataregistry.org/concepts/8594> ;
    reg:status <http://metadataregistry.org/uri/RegStatus/1001> ;
    a skos:Concept ;
    skos:definition "A single or composite sheet containing text and/or images, originally produced rolled, and intended to be unrolled a portion at a time for reading or viewing."@en ;
    skos:inScheme <http://rdaregistry.info/termList/RDATerms> ;
    skos:prefLabel "scroll"@en .

<http://rdaregistry.info/termList/RDATerms/1080>
    rdakit:toolkitDefinition "A manifestation that contains identifying information."@en ;
    rdakit:toolkitLabel "self-describing manifestation"@en ;
    reg:identifier <http://metadataregistry.org/concepts/8595> ;
    reg:status <http://metadataregistry.org/uri/RegStatus/1001> ;
    a skos:Concept ;
    skos:definition "A manifestation that contains identifying information."@en ;
    skos:inScheme <http://rdaregistry.info/termList/RDATerms> ;
    skos:prefLabel "self-describing manifestation"@en .

<http://rdaregistry.info/termList/RDATerms/1081>
    rdakit:toolkitDefinition "A group of separate manifestations related to one another by the fact that each manifestation bears, in addition to its own title proper, a collective title applying to the group as a whole with or without numbering or, a separately numbered sequence of volumes or issues within a series or serial."@en, "Grupo de recursos separados que estan relacionados entre si por el hecho de que cada recurso tiene, además de su título propiamente dicho, un título colectivo que se aplica al grupo como un todo. Los recursos individuales pueden estar o no numerados."@es ;
    rdakit:toolkitLabel "serie"@es, "serie"@it, "series"@en ;
    reg:identifier <http://metadataregistry.org/concepts/8596> ;
    reg:status <http://metadataregistry.org/uri/RegStatus/1001> ;
    a skos:Concept ;
    skos:definition "A group of separate manifestations related to one another by the fact that each manifestation bears, in addition to its own title proper, a collective title applying to the group as a whole with or without numbering or, a separately numbered sequence of volumes or issues within a series or serial."@en, "Grupo de recursos separados que estan relacionados entre si por el hecho de que cada recurso tiene, además de su título propiamente dicho, un título colectivo que se aplica al grupo como un todo. Los recursos individuales pueden estar o no numerados."@es ;
    skos:inScheme <http://rdaregistry.info/termList/RDATerms> ;
    skos:prefLabel "serie"@es, "serie"@it, "series"@en .

<http://rdaregistry.info/termList/RDATerms/1082>
    rdakit:toolkitDefinition "An added title page bearing a series title proper and usually, though not necessarily, other information about a series such as statement of responsibility, numeric designation, data relating to publication, title of the manifestation within the series."@en, "Frontespizio aggiunto che presenta il titolo proprio della serie e solitamente, benché non necessariamente, altre informazioni sulla serie."@it ;
    rdakit:toolkitLabel "frontespizio della serie"@it, "series title page"@en ;
    reg:identifier <http://metadataregistry.org/concepts/8597> ;
    reg:status <http://metadataregistry.org/uri/RegStatus/1001> ;
    a skos:Concept ;
    skos:definition "An added title page bearing a series title proper and usually, though not necessarily, other information about a series such as statement of responsibility, numeric designation, data relating to publication, title of the manifestation within the series."@en, "Frontespizio aggiunto che presenta il titolo proprio della serie e solitamente, benché non necessariamente, altre informazioni sulla serie."@it ;
    skos:inScheme <http://rdaregistry.info/termList/RDATerms> ;
    skos:prefLabel "frontespizio della serie"@it, "series title page"@en ;
    skos:related <http://rdaregistry.info/termList/RDATerms/1004>, <http://rdaregistry.info/termList/RDATerms/1095> .

<http://rdaregistry.info/termList/RDATerms/1083>
    rdakit:toolkitDefinition "A title of a legal work that is given either in the text of the work or in legal literature and that succinctly names the work and often reflects how it is popularly known."@en, "Titre d’une œuvre juridique qui est donné dans le texte même de l’œuvre ou dans la littérature juridique et qui nomme succinctement l’œuvre et reflète souvent comment elle est couramment connue."@fr ;
    rdakit:toolkitLabel "short title of a legal work"@en, "titre abrégé d’une œuvre juridique"@fr ;
    reg:identifier <http://metadataregistry.org/concepts/8598> ;
    reg:status <http://metadataregistry.org/uri/RegStatus/1001> ;
    a skos:Concept ;
    skos:definition "A title of a legal work that is given either in the text of the work or in legal literature and that succinctly names the work and often reflects how it is popularly known."@en, "Titre d’une œuvre juridique qui est donné dans le texte même de l’œuvre ou dans la littérature juridique et qui nomme succinctement l’œuvre et reflète souvent comment elle est couramment connue."@fr ;
    skos:inScheme <http://rdaregistry.info/termList/RDATerms> ;
    skos:prefLabel "short title of a legal work"@en, "titre abrégé d’une œuvre juridique"@fr .

<http://rdaregistry.info/termList/RDATerms/1084>
    rdakit:toolkitDefinition "A language that uses a system of manual, facial, and other body movements as the means of communication."@en, "Dans le contexte du contenu accessible, version en langue des signes du dialogue de la ressource affichée sur l’écran."@fr, "Nel contesto del contenuto accessibile, una versione nella lingua dei segni del dialogo della risorsa visualizzato sullo schermo."@it ;
    rdakit:toolkitLabel "langue des signes"@fr, "lingua dei segni"@it, "sign language"@en ;
    reg:identifier <http://metadataregistry.org/concepts/8599> ;
    reg:status <http://metadataregistry.org/uri/RegStatus/1001> ;
    a skos:Concept ;
    skos:definition "A language that uses a system of manual, facial, and other body movements as the means of communication."@en, "Dans le contexte du contenu accessible, version en langue des signes du dialogue de la ressource affichée sur l’écran."@fr, "Nel contesto del contenuto accessibile, una versione nella lingua dei segni del dialogo della risorsa visualizzato sullo schermo."@it ;
    skos:inScheme <http://rdaregistry.info/termList/RDATerms> ;
    skos:prefLabel "langue des signes"@fr, "lingua dei segni"@it, "sign language"@en .

<http://rdaregistry.info/termList/RDATerms/1085>
    rdakit:toolkitDefinition "A source of data from which a description, or portion thereof, is prepared."@en, "Fonte dei dati da cui si trae una descrizione (o una sua parte)."@it, "Fuente de los datos con los que se preparó una descripción (o una parte de ella)."@es ;
    rdakit:toolkitLabel "fonte d'informazione"@it, "fuente de información"@es, "source of information"@en ;
    reg:identifier <http://metadataregistry.org/concepts/8600> ;
    reg:status <http://metadataregistry.org/uri/RegStatus/1001> ;
    a skos:Concept ;
    skos:definition "A source of data from which a description, or portion thereof, is prepared."@en, "Fonte dei dati da cui si trae una descrizione (o una sua parte)."@it, "Fuente de los datos con los que se preparó una descripción (o una parte de ella)."@es ;
    skos:inScheme <http://rdaregistry.info/termList/RDATerms> ;
    skos:prefLabel "fonte d'informazione"@it, "fuente de información"@es, "source of information"@en .

<http://rdaregistry.info/termList/RDATerms/1086>
    rdakit:toolkitDefinition "A physical material or substance on which information or artistic content is stored."@en, "Materiale o sostanza fisica sul quale è memorizzata l'informazione o il contenuto artistico."@it ;
    rdakit:toolkitLabel "mezzo di memorizzazione"@it, "storage medium"@en ;
    reg:identifier <http://metadataregistry.org/concepts/8601> ;
    reg:status <http://metadataregistry.org/uri/RegStatus/1001> ;
    a skos:Concept ;
    skos:definition "A physical material or substance on which information or artistic content is stored."@en, "Materiale o sostanza fisica sul quale è memorizzata l'informazione o il contenuto artistico."@it ;
    skos:inScheme <http://rdaregistry.info/termList/RDATerms> ;
    skos:prefLabel "mezzo di memorizzazione"@it, "storage medium"@en ;
    skos:related <http://rdaregistry.info/termList/RDATerms/1016>, <http://rdaregistry.info/termList/RDATerms/1026>, <http://rdaregistry.info/termList/RDATerms/1058> .

<http://rdaregistry.info/termList/RDATerms/1087>
    rdakit:toolkitDefinition "A full or partial description of a related entity using the same data that would be recorded in RDA elements for a description of that related entity presented in an order specified by a recognized display standard."@en, "Descripción completa o parcial de un recurso que utiliza la misma estructura (i.e., el mismo orden de elementos) que se usa en el recurso que se describe."@es, "Description complète ou partielle d’une ressource selon la même structure (c’est-à-dire le même ordre des éléments) que celle utilisée pour la ressource décrite."@fr, "Descrizione comprensiva o parziale di una risorsa che riflette la stessa struttura (cioè lo stesso ordine di elementi) della risorsa descritta."@it ;
    rdakit:toolkitLabel "descripción estructurada"@es, "description structurée"@fr, "descrizione strutturata"@it, "structured description"@en ;
    reg:identifier <http://metadataregistry.org/concepts/8602> ;
    reg:status <http://metadataregistry.org/uri/RegStatus/1001> ;
    a skos:Concept ;
    skos:definition "A full or partial description of a related entity using the same data that would be recorded in RDA elements for a description of that related entity presented in an order specified by a recognized display standard."@en, "Descripción completa o parcial de un recurso que utiliza la misma estructura (i.e., el mismo orden de elementos) que se usa en el recurso que se describe."@es, "Description complète ou partielle d’une ressource selon la même structure (c’est-à-dire le même ordre des éléments) que celle utilisée pour la ressource décrite."@fr, "Descrizione comprensiva o parziale di una risorsa che riflette la stessa struttura (cioè lo stesso ordine di elementi) della risorsa descritta."@it ;
    skos:inScheme <http://rdaregistry.info/termList/RDATerms> ;
    skos:prefLabel "descripción estructurada"@es, "description structurée"@fr, "descrizione strutturata"@it, "structured description"@en .

<http://rdaregistry.info/termList/RDATerms/1088>
    rdakit:toolkitDefinition "A term, phrase, classification number, etc., that indicates what a work is about."@en, "Termi, ilmaus, luokka tms., joka ilmaisee mitä aihetta teos käsittelee."@fi ;
    rdakit:toolkitLabel "aihe"@fi, "subject"@en ;
    reg:identifier <http://metadataregistry.org/concepts/8603> ;
    reg:status <http://metadataregistry.org/uri/RegStatus/1001> ;
    a skos:Concept ;
    skos:definition "A term, phrase, classification number, etc., that indicates what a work is about."@en, "Termi, ilmaus, luokka tms., joka ilmaisee mitä aihetta teos käsittelee."@fi ;
    skos:inScheme <http://rdaregistry.info/termList/RDATerms> ;
    skos:prefLabel "aihe"@fi, "subject"@en .

<http://rdaregistry.info/termList/RDATerms/1089>
    rdakit:toolkitDefinition "A corporate body that forms an integral part of a larger body in relation to which it holds an inferior hierarchical rank."@en, "Collectivité qui fait intégralement partie d’une collectivité plus grande et qui, par rapport à celle-ci, occupe une position hiérarchique inférieure."@fr, "Ente che costituisce parte integrante di un ente più grande, rispetto al quale detiene un livello gerarchico inferiore."@it ;
    rdakit:toolkitLabel "collectivité subordonnée"@fr, "ente subordinato"@it, "subordinate body"@en ;
    reg:identifier <http://metadataregistry.org/concepts/8604> ;
    reg:status <http://metadataregistry.org/uri/RegStatus/1001> ;
    a skos:Concept ;
    skos:definition "A corporate body that forms an integral part of a larger body in relation to which it holds an inferior hierarchical rank."@en, "Collectivité qui fait intégralement partie d’une collectivité plus grande et qui, par rapport à celle-ci, occupe une position hiérarchique inférieure."@fr, "Ente che costituisce parte integrante di un ente più grande, rispetto al quale detiene un livello gerarchico inferiore."@it ;
    skos:inScheme <http://rdaregistry.info/termList/RDATerms> ;
    skos:prefLabel "collectivité subordonnée"@fr, "ente subordinato"@it, "subordinate body"@en .

<http://rdaregistry.info/termList/RDATerms/1090>
    rdakit:toolkitDefinition "A series within a series, that is, a series that always appears in conjunction with another, usually more comprehensive, series of which it forms a section. Its title may or may not be dependent on the title of the main series."@en, "Sarja, joka ilmestyy toisen (pää)sarjan osana. Alasarjalla voi olla itsenäinen tai epäitsenäinen, pääsarjan nimekkeestä riippuvainen nimeke."@fi, "Serie all'interno di una serie (cioè una serie che compare sempre insieme a un'altra serie, solitamente più ampia, di cui essa forma una sezione). Il suo titolo può essere o meno dipendente dal titolo della serie principale."@it, "Serie dentro de una serie (i.e., una serie que siempre aparece en conjunto con otra serie generalmente más amplia, de la cual aquella forma una sección). Su título puede o no dependiente del título de la serie principal."@es ;
    rdakit:toolkitLabel "alasarja"@fi, "sottoserie"@it, "subserie"@es, "subseries"@en ;
    reg:identifier <http://metadataregistry.org/concepts/8605> ;
    reg:status <http://metadataregistry.org/uri/RegStatus/1001> ;
    a skos:Concept ;
    skos:definition "A series within a series, that is, a series that always appears in conjunction with another, usually more comprehensive, series of which it forms a section. Its title may or may not be dependent on the title of the main series."@en, "Sarja, joka ilmestyy toisen (pää)sarjan osana. Alasarjalla voi olla itsenäinen tai epäitsenäinen, pääsarjan nimekkeestä riippuvainen nimeke."@fi, "Serie all'interno di una serie (cioè una serie che compare sempre insieme a un'altra serie, solitamente più ampia, di cui essa forma una sezione). Il suo titolo può essere o meno dipendente dal titolo della serie principale."@it, "Serie dentro de una serie (i.e., una serie que siempre aparece en conjunto con otra serie generalmente más amplia, de la cual aquella forma una sección). Su título puede o no dependiente del título de la serie principal."@es ;
    skos:inScheme <http://rdaregistry.info/termList/RDATerms> ;
    skos:prefLabel "alasarja"@fi, "sottoserie"@it, "subserie"@es, "subseries"@en .

<http://rdaregistry.info/termList/RDATerms/1091>
    rdakit:toolkitDefinition "A text displayed at the bottom of a moving image expression that is a translation or transcription of the dialogue or narrative."@en ;
    rdakit:toolkitLabel "subtitle"@en ;
    reg:identifier <http://metadataregistry.org/concepts/8606> ;
    reg:status <http://metadataregistry.org/uri/RegStatus/1001> ;
    a skos:Concept ;
    skos:definition "A text displayed at the bottom of a moving image expression that is a translation or transcription of the dialogue or narrative."@en ;
    skos:inScheme <http://rdaregistry.info/termList/RDATerms> ;
    skos:prefLabel "subtitle"@en .

<http://rdaregistry.info/termList/RDATerms/1092>
    rdakit:toolkitDefinition "A physical or logical subdivision of a unit."@en, "Subdivision physique ou logique d’une unité."@fr, "Suddivisione fisica o logica di una unità."@it, "Una subdivisión física o lógica de una unidad."@es ;
    rdakit:toolkitLabel "sottounità"@it, "sous-unité"@fr, "subunidad"@es, "subunit"@en ;
    reg:identifier <http://metadataregistry.org/concepts/8607> ;
    reg:status <http://metadataregistry.org/uri/RegStatus/1001> ;
    a skos:Concept ;
    skos:definition "A physical or logical subdivision of a unit."@en, "Subdivision physique ou logique d’une unité."@fr, "Suddivisione fisica o logica di una unità."@it, "Una subdivisión física o lógica de una unidad."@es ;
    skos:inScheme <http://rdaregistry.info/termList/RDATerms> ;
    skos:prefLabel "sottounità"@it, "sous-unité"@fr, "subunidad"@es, "subunit"@en ;
    skos:scopeNote "A subunit includes a page of a volume, a frame of a microfiche, a record in a digital file, etc."@en .

<http://rdaregistry.info/termList/RDATerms/1093>
    rdakit:toolkitDefinition "A list of a composer’s works, usually arranged in chronological order or by categories, with the theme given for each composition or for each section of large compositions."@en, "Elenco delle opere di un compositore, solitamente ordinato in ordine cronologico o per categorie, con il tema per ciascuna composizione o per ciascuna sezione delle grandi composizioni."@it ;
    rdakit:toolkitLabel "catalogo tematico"@it, "thematic index"@en ;
    reg:identifier <http://metadataregistry.org/concepts/8608> ;
    reg:status <http://metadataregistry.org/uri/RegStatus/1001> ;
    a skos:Concept ;
    skos:definition "A list of a composer’s works, usually arranged in chronological order or by categories, with the theme given for each composition or for each section of large compositions."@en, "Elenco delle opere di un compositore, solitamente ordinato in ordine cronologico o per categorie, con il tema per ciascuna composizione o per ciascuna sezione delle grandi composizioni."@it ;
    skos:inScheme <http://rdaregistry.info/termList/RDATerms> ;
    skos:prefLabel "catalogo tematico"@it, "thematic index"@en .

<http://rdaregistry.info/termList/RDATerms/1094>
    rdakit:toolkitDefinition "A frame or frames, usually found at the beginning of a manifestation produced on film, containing identifying textual information which is not part of the subject content of the work and which is used as a source of information in creating a description."@en, "Uno o più fotogrammi, solitamente all'inizio di una risorsa prodotta su pellicola (film, filmina, etc.) che contengono informazioni testuali identificative, non comprese nel contenuto di soggetto della risorsa, e che sono utilizzati come fonte delle informazioni nella creazione della descrizione."@it ;
    rdakit:toolkitLabel "fotogramma del titolo"@it, "title frame"@en ;
    reg:identifier <http://metadataregistry.org/concepts/8609> ;
    reg:status <http://metadataregistry.org/uri/RegStatus/1001> ;
    a skos:Concept ;
    skos:definition "A frame or frames, usually found at the beginning of a manifestation produced on film, containing identifying textual information which is not part of the subject content of the work and which is used as a source of information in creating a description."@en, "Uno o più fotogrammi, solitamente all'inizio di una risorsa prodotta su pellicola (film, filmina, etc.) che contengono informazioni testuali identificative, non comprese nel contenuto di soggetto della risorsa, e che sono utilizzati come fonte delle informazioni nella creazione della descrizione."@it ;
    skos:inScheme <http://rdaregistry.info/termList/RDATerms> ;
    skos:prefLabel "fotogramma del titolo"@it, "title frame"@en .

<http://rdaregistry.info/termList/RDATerms/1095>
    rdakit:toolkitDefinition "A page at the beginning of a manifestation bearing a title proper and usually, though not necessarily, a statement of responsibility and data relating to publication."@en, "Pagina all'inizio di una risorsa che reca il titolo proprio e solitamente, benché non necessariamente, la formulazione di responsabilità e la data di pubblicazione."@it ;
    rdakit:toolkitLabel "frontespizio"@it, "title page"@en ;
    reg:identifier <http://metadataregistry.org/concepts/8610> ;
    reg:status <http://metadataregistry.org/uri/RegStatus/1001> ;
    a skos:Concept ;
    skos:definition "A page at the beginning of a manifestation bearing a title proper and usually, though not necessarily, a statement of responsibility and data relating to publication."@en, "Pagina all'inizio di una risorsa che reca il titolo proprio e solitamente, benché non necessariamente, la formulazione di responsabilità e la data di pubblicazione."@it ;
    skos:inScheme <http://rdaregistry.info/termList/RDATerms> ;
    skos:prefLabel "frontespizio"@it, "title page"@en ;
    skos:related <http://rdaregistry.info/termList/RDATerms/1004>, <http://rdaregistry.info/termList/RDATerms/1082> ;
    skos:scopeNote "Facing pages or pages on successive leaves containing this information with or without repetition are considered collectively as a title page."@en, "Se queste informazioni sono date su due pagine a fronte o su pagine delle carte successive, con o senza ripetizioni, queste pagine si trattano nel loro insieme come frontespizio."@it .

<http://rdaregistry.info/termList/RDATerms/1096>
    rdakit:toolkitDefinition "A display of data about a digital manifestation that includes a title proper and usually, though not necessarily, a statement of responsibility and data relating to publication."@en, "Affichage de données relatives à une ressource numérique, comprenant le titre propre et, habituellement mais pas nécessairement, la mention de responsabilité et les données relatives à la publication."@fr, "Visualizzazione di dati su una risorsa digitale che include il titolo proprio e solitamente, benché non necessariamente, la formulazione di responsabilità e i dati sulla pubblicazione."@it ;
    rdakit:toolkitLabel "schermata del titolo"@it, "title screen"@en, "écran-titre"@fr ;
    reg:identifier <http://metadataregistry.org/concepts/8611> ;
    reg:status <http://metadataregistry.org/uri/RegStatus/1001> ;
    a skos:Concept ;
    skos:definition "A display of data about a digital manifestation that includes a title proper and usually, though not necessarily, a statement of responsibility and data relating to publication."@en, "Affichage de données relatives à une ressource numérique, comprenant le titre propre et, habituellement mais pas nécessairement, la mention de responsabilité et les données relatives à la publication."@fr, "Visualizzazione di dati su una risorsa digitale che include il titolo proprio e solitamente, benché non necessariamente, la formulazione di responsabilità e i dati sulla pubblicazione."@it ;
    skos:inScheme <http://rdaregistry.info/termList/RDATerms> ;
    skos:prefLabel "schermata del titolo"@it, "title screen"@en, "écran-titre"@fr .

<http://rdaregistry.info/termList/RDATerms/1097>
    rdakit:toolkitDefinition "Accordo interazionale concluso tra stati od organizzazioni internazionali in forma scritta e governato dal diritto internazionale."@it, "An international agreement concluded between states or international organizations in written form and governed by international law."@en, "Entente internationale sous forme écrite conclue entre des États ou des organisations internationales et régie par le droit international."@fr ;
    rdakit:toolkitLabel "traité"@fr, "trattato"@it, "treaty"@en ;
    reg:identifier <http://metadataregistry.org/concepts/8612> ;
    reg:status <http://metadataregistry.org/uri/RegStatus/1001> ;
    a skos:Concept ;
    skos:definition "Accordo interazionale concluso tra stati od organizzazioni internazionali in forma scritta e governato dal diritto internazionale."@it, "An international agreement concluded between states or international organizations in written form and governed by international law."@en, "Entente internationale sous forme écrite conclue entre des États ou des organisations internationales et régie par le droit international."@fr ;
    skos:inScheme <http://rdaregistry.info/termList/RDATerms> ;
    skos:prefLabel "traité"@fr, "trattato"@it, "treaty"@en ;
    skos:scopeNote "A treaty may be designated by various other terms such as agreement, concordat, convention, charter, declaration, exchange of notes, memorandum of understanding, modus vivendi, or protocol."@en, "Peut être désigné par une variété d’autres termes tels que accord, concordat, convention, charte, déclaration, échange de notes, entente, modus vivendi ou protocole."@fr, "Può essere designato da vari altri termini, come accordo, concordato, convenzione, statuto, dichiarazione, scambio di note, protocollo di intesa, modus vivendi, o protocollo."@it .

<http://rdaregistry.info/termList/RDATerms/1098>
    rdakit:toolkitDefinition "A form or genre or a generic term used frequently by different composers."@en, "Forma o genere (per esempio, capriccio, musica da camera, concerto, Magnificat, musica da film, notturno, opera musicale, musica sacra, suite, sonata a tre) o termine generico (per esempio, composizione, movimento, muziek, pezzo) utilizzati frequentemente da diversi compositori."@it, "Forme, genre ou terme générique utilisé fréquemment par différents compositeurs"@fr ;
    rdakit:toolkitLabel "tipo di composizione"@it, "type de composition"@fr, "type of composition"@en ;
    reg:identifier <http://metadataregistry.org/concepts/8613> ;
    reg:status <http://metadataregistry.org/uri/RegStatus/1001> ;
    a skos:Concept ;
    skos:definition "A form or genre or a generic term used frequently by different composers."@en, "Forma o genere (per esempio, capriccio, musica da camera, concerto, Magnificat, musica da film, notturno, opera musicale, musica sacra, suite, sonata a tre) o termine generico (per esempio, composizione, movimento, muziek, pezzo) utilizzati frequentemente da diversi compositori."@it, "Forme, genre ou terme générique utilisé fréquemment par différents compositeurs"@fr ;
    skos:inScheme <http://rdaregistry.info/termList/RDATerms> ;
    skos:prefLabel "tipo di composizione"@it, "type de composition"@fr, "type of composition"@en ;
    skos:scopeNote "Form or genre includes capriccio, chamber music, concerto, Magnificat, motion picture music, nocturne, opera, sacred music, suite, trio sonata. Generic term includes composition, movement, muziek, piece."@en .

<http://rdaregistry.info/termList/RDATerms/1099>
    rdakit:toolkitDefinition "A physical or logical constituent of a manifestation."@en, "Componente fisica o logica di una risorsa."@it, "Composant physique ou logique d’une ressource."@fr, "Un componente físico o lógico de un recurso."@es ;
    rdakit:toolkitLabel "unidad"@es, "unit"@en, "unità"@it, "unité"@fr ;
    reg:identifier <http://metadataregistry.org/concepts/8614> ;
    reg:status <http://metadataregistry.org/uri/RegStatus/1001> ;
    a skos:Concept ;
    skos:definition "A physical or logical constituent of a manifestation."@en, "Componente fisica o logica di una risorsa."@it, "Composant physique ou logique d’une ressource."@fr, "Un componente físico o lógico de un recurso."@es ;
    skos:inScheme <http://rdaregistry.info/termList/RDATerms> ;
    skos:prefLabel "unidad"@es, "unit"@en, "unità"@it, "unité"@fr ;
    skos:scopeNote "A unit includes a volume, audiocassette, film reel, a map, a digital file, etc."@en .

<http://rdaregistry.info/termList/RDATerms/1100>
    rdakit:toolkitDefinition "A full or partial description of an entity written as a phrase, sentence, paragraph, etc."@en, "Descripción total o parcial de un recurso escrito ccomo una frase, parágrafo, etc."@es, "Description complète ou partielle d’une ressource rédigée sous forme de phrase ou de paragraphe."@fr, "Descrizione comprensiva o parziale di una risorsa, redatta in forma di frase, paragrafo, etc."@it ;
    rdakit:toolkitLabel "descripción no estructurada"@es, "description non structurée"@fr, "descrizione non strutturata"@it, "unstructured description"@en ;
    reg:identifier <http://metadataregistry.org/concepts/8615> ;
    reg:status <http://metadataregistry.org/uri/RegStatus/1001> ;
    a skos:Concept ;
    skos:definition "A full or partial description of an entity written as a phrase, sentence, paragraph, etc."@en, "Descripción total o parcial de un recurso escrito ccomo una frase, parágrafo, etc."@es, "Description complète ou partielle d’une ressource rédigée sous forme de phrase ou de paragraphe."@fr, "Descrizione comprensiva o parziale di una risorsa, redatta in forma di frase, paragrafo, etc."@it ;
    skos:inScheme <http://rdaregistry.info/termList/RDATerms> ;
    skos:prefLabel "descripción no estructurada"@es, "description non structurée"@fr, "descrizione non strutturata"@it, "unstructured description"@en .

<http://rdaregistry.info/termList/RDATerms/1101>
    rdakit:toolkitDefinition "An integrating resource that consists of one or more base volumes updated by separate pages that are inserted, removed, and/or substituted."@en, "Risorsa integrativa costituita da uno o più volumi di base aggiornati mediante pagine fisicamente distinte inserite,rimosse e/o sostituite."@it ;
    rdakit:toolkitLabel "aggiornamento a fogli mobili"@it, "updating loose-leaf"@en ;
    reg:identifier <http://metadataregistry.org/concepts/8616> ;
    reg:status <http://metadataregistry.org/uri/RegStatus/1001> ;
    a skos:Concept ;
    skos:definition "An integrating resource that consists of one or more base volumes updated by separate pages that are inserted, removed, and/or substituted."@en, "Risorsa integrativa costituita da uno o più volumi di base aggiornati mediante pagine fisicamente distinte inserite,rimosse e/o sostituite."@it ;
    skos:inScheme <http://rdaregistry.info/termList/RDATerms> ;
    skos:prefLabel "aggiornamento a fogli mobili"@it, "updating loose-leaf"@en .

<http://rdaregistry.info/termList/RDATerms/1102>
    rdakit:toolkitDefinition "Alternativa al punto d'accesso autorizzato che rappresenta un'entità."@it, "Alternativa al punto de acceso autorizado que representa una entidad."@es, "An alternative to an authorized access point representing an entity."@en, "Autre forme du point d’accès autorisé représentant une entité."@fr ;
    rdakit:toolkitLabel "punto d'accesso variante"@it, "punto de acceso variante"@es, "variant access point"@en, "variante de point d’accès"@fr ;
    reg:identifier <http://metadataregistry.org/concepts/8617> ;
    reg:status <http://metadataregistry.org/uri/RegStatus/1001> ;
    a skos:Concept ;
    skos:broader <http://rdaregistry.info/termList/RDATerms/1001> ;
    skos:definition "Alternativa al punto d'accesso autorizzato che rappresenta un'entità."@it, "Alternativa al punto de acceso autorizado que representa una entidad."@es, "An alternative to an authorized access point representing an entity."@en, "Autre forme du point d’accès autorisé représentant une entité."@fr ;
    skos:inScheme <http://rdaregistry.info/termList/RDATerms> ;
    skos:prefLabel "punto d'accesso variante"@it, "punto de acceso variante"@es, "variant access point"@en, "variante de point d’accès"@fr .

<http://rdaregistry.info/termList/RDATerms/1103>
    rdakit:toolkitDefinition "A name or form of name by which an entity is known that differs from the name or form of name chosen as a preferred name for that entity."@en, "Nom ou forme de nom sous laquelle une personne, famille ou collectivité est connue et qui diffère du nom ou de la forme de nom choisie comme nom privilégié pour cette personne, famille ou collectivité."@fr, "Nombre o una forma de un nombre mediante el cual se conoce a una entidad que difiere del nombre o forma del nombre escogido como el nombre preferido para esa entidad."@es, "Nome o forma del nome con cui un'entità è conosciuta, diverso dal nome o dalla forma del nome scelti come nome preferito per quella entità."@it ;
    rdakit:toolkitLabel "nome variante"@it, "variant name"@en, "variante de nom"@fr, "variante del nombre"@es ;
    reg:identifier <http://metadataregistry.org/concepts/8618> ;
    reg:status <http://metadataregistry.org/uri/RegStatus/1001> ;
    a skos:Concept ;
    skos:definition "A name or form of name by which an entity is known that differs from the name or form of name chosen as a preferred name for that entity."@en, "Nom ou forme de nom sous laquelle une personne, famille ou collectivité est connue et qui diffère du nom ou de la forme de nom choisie comme nom privilégié pour cette personne, famille ou collectivité."@fr, "Nombre o una forma de un nombre mediante el cual se conoce a una entidad que difiere del nombre o forma del nombre escogido como el nombre preferido para esa entidad."@es, "Nome o forma del nome con cui un'entità è conosciuta, diverso dal nome o dalla forma del nome scelti come nome preferito per quella entità."@it ;
    skos:inScheme <http://rdaregistry.info/termList/RDATerms> ;
    skos:prefLabel "nome variante"@it, "variant name"@en, "variante de nom"@fr, "variante del nombre"@es .

<http://rdaregistry.info/termList/RDATerms/1104>
    rdakit:toolkitDefinition "A length of magnetic tape on which are recorded electrical signals that can be converted to images using video playback equipment."@en, "Métrage de bande magnétique sur laquelle est enregistré un signal électrique qui peut être converti en images à l’aide d’un équipement de lecture vidéo."@fr ;
    rdakit:toolkitLabel "bande vidéo"@fr, "video tape"@en ;
    reg:identifier <http://metadataregistry.org/concepts/8619> ;
    reg:status <http://metadataregistry.org/uri/RegStatus/1001> ;
    a skos:Concept ;
    skos:definition "A length of magnetic tape on which are recorded electrical signals that can be converted to images using video playback equipment."@en, "Métrage de bande magnétique sur laquelle est enregistré un signal électrique qui peut être converti en images à l’aide d’un équipement de lecture vidéo."@fr ;
    skos:inScheme <http://rdaregistry.info/termList/RDATerms> ;
    skos:prefLabel "bande vidéo"@fr, "video tape"@en .

<http://rdaregistry.info/termList/RDATerms/1105>
    rdakit:toolkitDefinition "A named structured list of representations of controlled values for elements."@en, "Liste structurée et nommée de représentations de valeurs contrôlées pour les éléments"@fr, "Una lista strutturata identificata di rappresentazioni di valori controllati per gli elementi (per es., le liste di termini incluse in RDA o i vocabolari di valori ad esse corrispondenti con gli URI assegnati nel RDA Registry, liste di codici ISO, terminologie standard)."@it ;
    rdakit:toolkitLabel "schema di codifica di vocabolario"@it, "schéma d’encodage de vocabulaire"@fr, "vocabulary encoding scheme"@en ;
    reg:identifier <http://metadataregistry.org/concepts/8620> ;
    reg:status <http://metadataregistry.org/uri/RegStatus/1001> ;
    a skos:Concept ;
    skos:definition "A named structured list of representations of controlled values for elements."@en, "Liste structurée et nommée de représentations de valeurs contrôlées pour les éléments"@fr, "Una lista strutturata identificata di rappresentazioni di valori controllati per gli elementi (per es., le liste di termini incluse in RDA o i vocabolari di valori ad esse corrispondenti con gli URI assegnati nel RDA Registry, liste di codici ISO, terminologie standard)."@it ;
    skos:inScheme <http://rdaregistry.info/termList/RDATerms> ;
    skos:prefLabel "schema di codifica di vocabolario"@it, "schéma d’encodage de vocabulaire"@fr, "vocabulary encoding scheme"@en ;
    skos:scopeNote "A vocabulary encoding scheme includes an internal RDA list of terms or their corresponding value vocabularies with assigned URIs in the RDA Registry, an ISO code list, a standard terminology, etc."@en .

<http://rdaregistry.info/termList/RDATerms/1106>
    rdakit:toolkitDefinition "A separately issued part of a manifestation, usually representing a particular subject category within the larger manifestation and identified by a designation that may be a topic, or an alphabetic or numeric designation, or a combination of these."@en ;
    rdakit:toolkitLabel "section"@en ;
    reg:identifier <http://metadataregistry.org/concepts/8621> ;
    reg:status <http://metadataregistry.org/uri/RegStatus/1001> ;
    a skos:Concept ;
    skos:definition "A separately issued part of a manifestation, usually representing a particular subject category within the larger manifestation and identified by a designation that may be a topic, or an alphabetic or numeric designation, or a combination of these."@en ;
    skos:inScheme <http://rdaregistry.info/termList/RDATerms> ;
    skos:prefLabel "section"@en .

<http://rdaregistry.info/termList/RDATerms/1107>
    rdakit:toolkitDefinition "A resource related to another resource."@en ;
    rdakit:toolkitLabel "related resource"@en ;
    reg:identifier <http://metadataregistry.org/concepts/8622> ;
    reg:status <http://metadataregistry.org/uri/RegStatus/1001> ;
    a skos:Concept ;
    skos:definition "A resource related to another resource."@en ;
    skos:inScheme <http://rdaregistry.info/termList/RDATerms> ;
    skos:prefLabel "related resource"@en .

