@prefix rdf: <http://www.w3.org/1999/02/22-rdf-syntax-ns#> .
@prefix dc: <http://purl.org/dc/elements/1.1/> .
@prefix reg: <http://metadataregistry.org/uri/profile/regap/> .
@prefix skos: <http://www.w3.org/2004/02/skos/core#> .

<http://metadataregistry.org/uri/RegStatus/1001>
    a skos:Concept ;
    skos:prefLabel "Published"@en .

<http://rdaregistry.info/termList/rofit>
    dc:title "ROF Intermediation Tool" ;
    a skos:ConceptScheme .

<http://rdaregistry.info/termList/rofit/T1001>
    reg:identifier <http://metadataregistry.org/concepts/6953> ;
    reg:status <http://metadataregistry.org/uri/RegStatus/1001> ;
    a skos:Concept ;
    skos:definition "A device that magnifies microforms for reading with the unaided eye."@en ;
    skos:inScheme <http://rdaregistry.info/termList/rofit> ;
    skos:prefLabel "microform reader"@en .

<http://rdaregistry.info/termList/rofit/T1002>
    reg:identifier <http://metadataregistry.org/concepts/6954> ;
    reg:status <http://metadataregistry.org/uri/RegStatus/1001> ;
    a skos:Concept ;
    skos:definition "An instrument that magnifies objects by means of a lens or lenses so as to reveal details invisible to the naked eye."@en ;
    skos:inScheme <http://rdaregistry.info/termList/rofit> ;
    skos:prefLabel "microscope"@en .

<http://rdaregistry.info/termList/rofit/T1003>
    reg:identifier <http://metadataregistry.org/concepts/6955> ;
    reg:status <http://metadataregistry.org/uri/RegStatus/1001> ;
    a skos:Concept ;
    skos:definition "An optical device containing a light source and lens system for projecting an image on a screen or other surface."@en ;
    skos:inScheme <http://rdaregistry.info/termList/rofit> ;
    skos:prefLabel "projector"@en .

<http://rdaregistry.info/termList/rofit/T1004>
    reg:identifier <http://metadataregistry.org/concepts/6956> ;
    reg:status <http://metadataregistry.org/uri/RegStatus/1001> ;
    a skos:Concept ;
    skos:definition "An optical device with two lenses enabling each eye to see a separate image of essentially the same content to give the effect of three-dimensions."@en ;
    skos:inScheme <http://rdaregistry.info/termList/rofit> ;
    skos:prefLabel "stereoscope"@en .

<http://rdaregistry.info/termList/rofit/T1005>
    reg:identifier <http://metadataregistry.org/concepts/6957> ;
    reg:status <http://metadataregistry.org/uri/RegStatus/1001> ;
    a skos:Concept ;
    skos:definition "A device designed to play audio recordings."@en ;
    skos:inScheme <http://rdaregistry.info/termList/rofit> ;
    skos:prefLabel "audio player"@en .

<http://rdaregistry.info/termList/rofit/T1006>
    reg:identifier <http://metadataregistry.org/concepts/6958> ;
    reg:status <http://metadataregistry.org/uri/RegStatus/1001> ;
    a skos:Concept ;
    skos:definition "A device designed to play audiovisual recordings."@en ;
    skos:inScheme <http://rdaregistry.info/termList/rofit> ;
    skos:prefLabel "audiovisual player"@en .

<http://rdaregistry.info/termList/rofit/T1007>
    reg:identifier <http://metadataregistry.org/concepts/6959> ;
    reg:status <http://metadataregistry.org/uri/RegStatus/1001> ;
    a skos:Concept ;
    skos:definition "A device designed to perform prescribed sequences of operations on electronic data."@en ;
    skos:inScheme <http://rdaregistry.info/termList/rofit> ;
    skos:prefLabel "computer"@en .

<http://rdaregistry.info/termList/rofit/T1008>
    reg:identifier <http://metadataregistry.org/concepts/6960> ;
    reg:status <http://metadataregistry.org/uri/RegStatus/1001> ;
    a skos:Concept ;
    skos:definition "No intermediation tool is required (i.e., the content of the resource is directly and adequately perceivable through one or more of the human senses)."@en ;
    skos:inScheme <http://rdaregistry.info/termList/rofit> ;
    skos:prefLabel "not required"@en .

